

To calculate the definite integral \(\int_0^\infty \frac{1}{e^x + 1} \, dx\), we proceed as follows:

### Step 1: Analytic Solution
First, rewrite the integrand by multiplying numerator and denominator by \(e^{-x}\):
\[
\frac{1}{e^x + 1} = \frac{e^{-x}}{1 + e^{-x}}.
\]
For \(x > 0\), \(e^{-x} < 1\), so we can expand \(\frac{1}{1 + e^{-x}}\) as a geometric series:
\[
\frac{1}{1 + e^{-x}} = \sum_{n=0}^\infty (-1)^n e^{-nx}.
\]
Substituting this into the integrand gives:
\[
\frac{e^{-x}}{1 + e^{-x}} = e^{-x} \sum_{n=0}^\infty (-1)^n e^{-nx} = \sum_{n=0}^\infty (-1)^n e^{-(n+1)x}.
\]
Interchanging the sum and integral (justified by uniform convergence), we integrate term-by-term:
\[
\int_0^\infty \frac{1}{e^x + 1} \, dx = \sum_{n=0}^\infty (-1)^n \int_0^\infty e^{-(n+1)x} \, dx.
\]
The integral \(\int_0^\infty e^{-ax} \, dx = \frac{1}{a}\) for \(a > 0\). Here, \(a = n+1\), so:
\[
\int_0^\infty e^{-(n+1)x} \, dx = \frac{1}{n+1}.
\]
Thus, the integral becomes:
\[
\sum_{n=0}^\infty \frac{(-1)^n}{n+1}.
\]
Reindexing with \(k = n+1\), this sum is:
\[
\sum_{k=1}^\infty \frac{(-1)^{k-1}}{k}.
\]
This is the alternating harmonic series, which converges to \(\ln 2\).

### Step 2: Numerical Approximation
The numerical value of \(\ln 2\) is approximately \(0.69314718056\). Rounded to 10 decimal places, this is \(0.6931471806\).

{"answer": "\(\ln 2\)", "numerical_answer": "0.6931471806"}