

To solve the definite integral \(\int_{1.0}^\infty x(x^2-1.0^2)^{2-3/2}e^{-0.5^2x^2}H_{2 \times 2}(0.5x)dx\), we follow these steps:

### Step 1: Simplify the Integrand
The exponent \(2 - 3/2 = 1/2\), so \((x^2 - 1)^{1/2} = \sqrt{x^2 - 1}\). The integrand becomes:
\[
x \sqrt{x^2 - 1} e^{-0.25x^2} H_4(0.5x)
\]
where \(H_4(z)\) is the 4th Hermite polynomial, \(H_4(z) = 16z^4 - 48z^2 + 12\).

### Step 2: Substitution
Let \(t = 0.5x\), so \(x = 2t\), \(dx = 2dt\). The limits change from \(x=1\) ( \(t=0.5\) ) to \(x \to \infty\) ( \(t \to \infty\) ). Substituting:
- \(x = 2t\), \(x^2 - 1 = 4t^2 - 1\), \(\sqrt{x^2 - 1} = \sqrt{4t^2 - 1}\)
- \(e^{-0.25x^2} = e^{-t^2}\), \(H_4(0.5x) = H_4(t) = 16t^4 - 48t^2 + 12\)

The integral becomes:
\[
4 \int_{0.5}^\infty t \sqrt{4t^2 - 1} e^{-t^2} (16t^4 - 48t^2 + 12) dt
\]

### Step 3: Further Substitution
Let \(u = 4t^2 - 1\), so \(du = 8t dt\) ( \(t dt = du/8\) ), \(t^2 = (u + 1)/4\), and \(e^{-t^2} = e^{-(u + 1)/4} = e^{-1/4}e^{-u/4}\). The limits change from \(t=0.5\) ( \(u=0\) ) to \(t \to \infty\) ( \(u \to \infty\) ). The polynomial \(16t^4 - 48t^2 + 12\) simplifies to \(u^2 - 10u + 1\) in terms of \(u\).

The integral transforms to:
\[
0.5 e^{-1/4} \int_{0}^\infty u^{1/2} (u^2 - 10u + 1) e^{-u/4} du
\]

### Step 4: Gamma Function Evaluation
The integral \(\int_{0}^\infty u^{1/2} (u^2 - 10u + 1) e^{-u/4} du\) is evaluated using Gamma functions:
\[
\int_0^\infty u^{s-1} e^{-au} du = \frac{\Gamma(s)}{a^s}
\]
For \(s = 7/2, 5/2, 3/2\) and \(a = 1/4\), the integral simplifies to \(4\sqrt{\pi}\).

### Step 5: Final Result
Combining constants, the exact integral is:
\[
2 e^{-1/4} \sqrt{\pi}
\]

### Numerical Approximation
Using \(e^{-1/4} \approx 0.77880078307\) and \(\sqrt{\pi} \approx 1.77245385091\), the numerical value is approximately \(2.7607774581\).

{"answer": "2 e^{-1/4} \sqrt{\pi}", "numerical_answer": "2.7607774581"}