

To calculate the definite integral \(\int_0^\infty \frac{\tanh(x)}{e^x} \, dx\), we proceed as follows:

### Step 1: Simplify the integrand using hyperbolic identities
Recall that \(\tanh(x) = \frac{e^x - e^{-x}}{e^x + e^{-x}}\). Substituting this into the integrand:
\[
\frac{\tanh(x)}{e^x} = \frac{e^x - e^{-x}}{(e^x + e^{-x})e^x} = \frac{1 - e^{-2x}}{e^x + e^{-x}}.
\]

### Step 2: Substitution to simplify the integral
Let \(u = e^{-x}\), so \(du = -e^{-x} \, dx = -u \, dx\) (or \(dx = -\frac{du}{u}\)). When \(x = 0\), \(u = 1\); as \(x \to \infty\), \(u \to 0\). Rewriting the integrand in terms of \(u\):
\[
\frac{1 - e^{-2x}}{e^x + e^{-x}} = \frac{1 - u^2}{u^{-1} + u} = \frac{(1 - u^2)u}{1 + u^2}.
\]
The integral becomes:
\[
\int_0^\infty \frac{\tanh(x)}{e^x} \, dx = \int_1^0 \frac{(1 - u^2)u}{1 + u^2} \left(-\frac{du}{u}\right) = \int_0^1 \frac{1 - u^2}{1 + u^2} \, du.
\]

### Step 3: Evaluate the simplified integral
Split the integrand:
\[
\frac{1 - u^2}{1 + u^2} = \frac{(1 + u^2) - 2u^2}{1 + u^2} = 1 - \frac{2u^2}{1 + u^2} = -1 + \frac{2}{1 + u^2}.
\]
Integrate term by term:
\[
\int_0^1 \left(-1 + \frac{2}{1 + u^2}\right) du = \int_0^1 -1 \, du + 2 \int_0^1 \frac{1}{1 + u^2} \, du.
\]
The first integral is:
\[
\int_0^1 -1 \, du = -[u]_0^1 = -1.
\]
The second integral uses \(\int \frac{1}{1 + u^2} \, du = \arctan(u)\):
\[
2 \int_0^1 \frac{1}{1 + u^2} \, du = 2[\arctan(u)]_0^1 = 2\left(\frac{\pi}{4} - 0\right) = \frac{\pi}{2}.
\]
Combining these results:
\[
\int_0^1 \frac{1 - u^2}{1 + u^2} \, du = -1 + \frac{\pi}{2}.
\]

### Step 4: Numerical approximation
The exact result is \(\frac{\pi}{2} - 1\). Numerically, \(\pi \approx 3.141592653589793\), so:
\[
\frac{\pi}{2} - 1 \approx 1.5707963267948966 - 1 = 0.5707963267948966.
\]
Rounded to 10 decimal places, this is \(0.5707963268\).

{"answer": "\(\frac{\pi}{2} - 1\)", "numerical_answer": "0.5707963268"}