To evaluate the definite integral

$$
\int_0^2 x^{-1/2}(2 - x)^{1/2} \sqrt{1 - 0.5x(2 - x)} \, dx,
$$

we begin by simplifying the integrand and identifying a suitable substitution.

---

### **Step 1: Simplify the Integrand**

The term inside the square root simplifies as follows:

$$
1 - 0.5x(2 - x) = 1 - x + \frac{x^2}{2} = \frac{x^2 - 2x + 2}{2}.
$$

So the integrand becomes:

$$
x^{-1/2}(2 - x)^{1/2} \sqrt{\frac{x^2 - 2x + 2}{2}}.
$$

This can be rewritten as:

$$
\frac{1}{\sqrt{2}} \cdot x^{-1/2}(2 - x)^{1/2} \sqrt{x^2 - 2x + 2}.
$$

---

### **Step 2: Substitution**

Let us perform the substitution $ x = t + 1 $, so that $ dx = dt $, and the limits become $ t = -1 $ to $ t = 1 $.

Then:

- $ x = t + 1 \Rightarrow x^{-1/2} = (t + 1)^{-1/2} $,
- $ 2 - x = 1 - t \Rightarrow (2 - x)^{1/2} = (1 - t)^{1/2} $,
- $ x^2 - 2x + 2 = (t + 1)^2 - 2(t + 1) + 2 = t^2 + 1 $.

So the integrand becomes:

$$
\frac{1}{\sqrt{2}} \cdot (t + 1)^{-1/2}(1 - t)^{1/2} \sqrt{t^2 + 1}.
$$

Thus, the integral becomes:

$$
\frac{1}{\sqrt{2}} \int_{-1}^{1} (t + 1)^{-1/2}(1 - t)^{1/2} \sqrt{t^2 + 1} \, dt.
$$

---

### **Step 3: Exploit Symmetry**

We can exploit the symmetry of the integrand about $ t = 0 $. The function is even in $ t $, so:

$$
\int_{-1}^{1} f(t) \, dt = 2 \int_0^1 f(t) \, dt.
$$

This simplifies the integral to:

$$
\frac{2}{\sqrt{2}} \int_0^1 (t + 1)^{-1/2}(1 - t)^{1/2} \sqrt{t^2 + 1} \, dt.
$$

Further simplification gives:

$$
\sqrt{2} \int_0^1 \sqrt{\frac{1 - t}{1 + t}} \cdot \sqrt{t^2 + 1} \, dt.
$$

---

### **Step 4: Trigonometric Substitution**

Let $ t = \sin\theta $, so $ dt = \cos\theta \, d\theta $, and when $ t = 0 $, $ \theta = 0 $; $ t = 1 $, $ \theta = \frac{\pi}{2} $.

Then:

- $ \sqrt{\frac{1 - t}{1 + t}} = \sqrt{\frac{1 - \sin\theta}{1 + \sin\theta}} = \tan\left(\frac{\pi}{4} - \frac{\theta}{2}\right) $,
- $ \sqrt{t^2 + 1} = \sqrt{\sin^2\theta + 1} = \sqrt{1 + \sin^2\theta} $,
- $ dt = \cos\theta \, d\theta $.

The integral becomes:

$$
\sqrt{2} \int_0^{\pi/2} \tan\left(\frac{\pi}{4} - \frac{\theta}{2}\right) \cdot \sqrt{1 + \sin^2\theta} \cdot \cos\theta \, d\theta.
$$

This form is not elementary, but it can be related to the **complete elliptic integral of the second kind**.

---

### **Step 5: Final Analytical Result**

Through a series of transformations and standard results, the integral simplifies to:

$$