I'll solve the definite integral $\int\limits_0^\infty e^{-3.0x}\left[\frac1{1.0x}I_0(1.0x)-K_1(1.0x)\right]dx$ step by step.

## Step 1: Identify the special functions
In this integral, we have:
- $I_0(x)$ is the modified Bessel function of the first kind of order 0
- $K_1(x)$ is the modified Bessel function of the second kind of order 1

## Step 2: Recall useful Bessel function properties
For simplicity, I'll denote $a = 1.0$ and $b = 3.0$ in the calculations.

The expression $\frac{1}{x}I_0(x) - K_1(x)$ appears in our integral. This combination can be related to Laplace transforms.

## Step 3: Apply Laplace transform properties
Let's denote $f(x) = \frac{1}{x}I_0(x) - K_1(x)$

The Laplace transform of $f(x)$ is known to be:
$\mathcal{L}\{f(x)\}(s) = \int_0^\infty e^{-sx}f(x)dx = \frac{1}{\sqrt{s^2-1}} - \frac{1}{s}$

Therefore, our integral $\int_0^\infty e^{-bx}f(ax)dx$ can be evaluated using the scaling property of Laplace transforms.

## Step 4: Use the scaling property
If $\mathcal{L}\{f(x)\}(s) = F(s)$, then $\mathcal{L}\{f(ax)\}(s) = \frac{1}{a}F(\frac{s}{a})$

So our integral becomes:
$\int_0^\infty e^{-bx}f(ax)dx = \frac{1}{a}\mathcal{L}\{f(ax)\}(b) = \frac{1}{a}F(\frac{b}{a})$

With $F(s) = \frac{1}{\sqrt{s^2-1}} - \frac{1}{s}$, we get:
$\frac{1}{a}F(\frac{b}{a}) = \frac{1}{a}\left[\frac{1}{\sqrt{(\frac{b}{a})^2-1}} - \frac{1}{\frac{b}{a}}\right] = \frac{1}{a}\left[\frac{1}{\sqrt{\frac{b^2-a^2}{a^2}}} - \frac{a}{b}\right]$

Simplifying:
$= \frac{1}{a}\left[\frac{a}{\sqrt{b^2-a^2}} - \frac{a}{b}\right] = \frac{1}{\sqrt{b^2-a^2}} - \frac{1}{b}$

## Step 5: Substitute back our values
With $a = 1.0$ and $b = 3.0$:
$\int_0^\infty e^{-3.0x}\left[\frac{1}{1.0x}I_0(1.0x)-K_1(1.0x)\right]dx = \frac{1}{\sqrt{3.0^2-1.0^2}} - \frac{1}{3.0}$

$= \frac{1}{\sqrt{9-1}} - \frac{1}{3} = \frac{1}{\sqrt{8}} - \frac{1}{3} = \frac{1}{2\sqrt{2}} - \frac{1}{3}$

## Step 6: Calculate the exact value
$\frac{1}{2\sqrt{2}} - \frac{1}{3} = \frac{3}{6\sqrt{2}} - \frac{2\sqrt{2}}{6\sqrt{2}} = \frac{3-2\sqrt{2}}{6\sqrt{2}} = \frac{3-2\sqrt{2}}{6\sqrt{2}} \cdot \frac{\sqrt{2}}{\sqrt{2}} = \frac{3\sqrt{2}-4}{6\cdot 2} = \frac{3\sqrt{2}-4}{12}$

## Step 7: Numerical approximation
$\frac{3\sqrt{2}-4}{12} = \frac{3 \cdot 1.4142135624 - 4}{12} \approx \frac{4.2426406871 - 4}{12} \approx \frac{0.2426406871}{12} \approx 0.0202200573$

When calculated more precisely, the numerical value is:
$\frac{3\sqrt{2}-4}{12} = 0.0202200573$

{"answer": "\\frac{3\\sqrt{2}-4}{12}", "numerical_answer": "0.0202200573"}