# Evaluating $\int_0^1e^{e^x}-e^{e^x-x}\:dx$

I'll evaluate this definite integral step-by-step.

## Step 1: Simplify the integrand

First, let's observe a potential simplification in the integrand:
$e^{e^x}-e^{e^x-x}$

Note that $e^{e^x-x} = e^{e^x} \cdot e^{-x} = \frac{e^{e^x}}{e^x}$

So the integrand becomes:
$e^{e^x}-\frac{e^{e^x}}{e^x} = e^{e^x} - \frac{e^{e^x}}{e^x} = e^{e^x}\left(1-\frac{1}{e^x}\right) = e^{e^x}\left(\frac{e^x-1}{e^x}\right) = e^{e^x}\frac{e^x-1}{e^x}$

This simplifies to:
$e^{e^x} \cdot \frac{e^x-1}{e^x} = e^{e^x} \cdot (1-e^{-x})$

## Step 2: Let's make a substitution

Let $u = e^x$, which means $x = \ln(u)$ and $dx = \frac{1}{u}du$

When $x = 0$, $u = e^0 = 1$
When $x = 1$, $u = e^1 = e$

The integrand transforms to:
$e^{e^x} \cdot (1-e^{-x}) = e^u \cdot (1-\frac{1}{u})$

And the integral becomes:
$\int_0^1 e^{e^x}-e^{e^x-x}\:dx = \int_1^e e^u \cdot (1-\frac{1}{u}) \cdot \frac{1}{u}du = \int_1^e \frac{e^u}{u} - \frac{e^u}{u^2}du$

## Step 3: Evaluate the transformed integral

Let's define:
- $I_1 = \int_1^e \frac{e^u}{u}du$
- $I_2 = \int_1^e \frac{e^u}{u^2}du$

So our integral is $I_1 - I_2$

For $I_2$, we can use integration by parts:
Let $v = \frac{1}{u^2}$ and $dw = e^u du$
Then $dv = -\frac{2}{u^3}du$ and $w = e^u$

By parts: $\int v \cdot dw = v \cdot w - \int w \cdot dv$

$I_2 = \int_1^e \frac{e^u}{u^2}du = \left.\frac{e^u}{u^2}\right|_1^e - \int_1^e e^u \cdot (-\frac{2}{u^3})du = \left.\frac{e^u}{u^2}\right|_1^e + 2\int_1^e \frac{e^u}{u^3}du$

The evaluation at bounds gives:
$\left.\frac{e^u}{u^2}\right|_1^e = \frac{e^e}{e^2} - \frac{e^1}{1^2} = \frac{e^e}{e^2} - e = \frac{e^{e-2} - e}{}$

For the remaining integral, we need further integration by parts. However, this approach becomes quite complex.

## Step 4: Alternative approach

Let's try a different approach by directly evaluating the original integral.

Setting $u = e^x$ as before, the integral becomes:
$\int_0^1 e^{e^x}-e^{e^x-x}\:dx = \int_1^e \frac{e^u - e^{u-\ln u}}{u}du$

But $e^{u-\ln u} = e^u \cdot e^{-\ln u} = e^u \cdot \frac{1}{u} = \frac{e^u}{u}$

So our integral simplifies to:
$\int_1^e \frac{e^u - \frac{e^u}{u}}{u}du = \int_1^e \frac{e^u}{u} - \frac{e^u}{u^2}du$

I need to take another approach to solve this.

## Step 5: Using the fundamental theorem of calculus

Looking at the original integrand more carefully: $e^{e^x}-e^{e^x-x}$

Let's consider a function $F(x) = e^{e^x-x}$

Then $F'(x) = e^{e^x-x} \cdot (e^x - 1)$

Rearranging:
$F'(x) = e^{e^x-x} \cdot e^x - e^{e^x-x} = e^{e^x} - e^{e^x-x}$

This is exactly our integrand! So the integral is:
$\int_0^1 e^{e^x}-e^{e^x-x}\:dx = \int_0^1 F'(x)dx = F(1) - F(0) = e^{e^1-1} - e^{e^0-0} = e^{e-1} - e^{1} = e^{e-1} - e$

## Step 6: Numerical approximation

The exact answer is $e^{e-1} - e$

Calculating numerically:
- $e ≈ 2.7182818284...$
- $e-1 ≈ 1.7182818284...$
- $e^{e-1} ≈ 5.5374809465...$
- $e^{e-1} - e ≈ 5.5374809465... - 2.7182818284... ≈ 2.8191991181...$

Rounded to 10 decimal places: $2.8191991181$

{"answer": "e^{e-1} - e", "numerical_answer": "2.8191991181"}