Let's compute the integral:
\[
I = \int_0^1 \arccos x \, J_1(2x) \, dx
\]

**Step 1: Substitution**

Let \( x = \cos\theta \), so as \( x \) goes from 0 to 1, \( \theta \) goes from \( \arccos 1 = 0 \) to \( \arccos 0 = \frac{\pi}{2} \).

- \( dx = -\sin\theta \, d\theta \)
- \( \arccos x = \theta \)
- \( J_1(2x) = J_1(2\cos\theta) \)

So,
\[
I = \int_{x=0}^{x=1} \arccos x \, J_1(2x) \, dx = \int_{\theta=\frac{\pi}{2}}^{\theta=0} \theta \, J_1(2\cos\theta) \, (-\sin\theta) \, d\theta
\]
\[
= \int_{0}^{\frac{\pi}{2}} \theta \, J_1(2\cos\theta) \, \sin\theta \, d\theta
\]

**Step 2: Integration by Parts**

Let \( u = \theta \), \( dv = J_1(2\cos\theta)\sin\theta d\theta \).

But let's try integrating by parts with respect to \(\theta\):

Let \( u = \theta \), \( dv = J_1(2\cos\theta)\sin\theta d\theta \).

Then \( du = d\theta \).

Let us try to find \( v \):

Let’s try to write \( J_1(2\cos\theta)\sin\theta \) in a more manageable form.

Alternatively, let's try to use the integral representation of \( J_1 \):

But perhaps a better approach is to use the series expansion for \( J_1(2x) \):

\[
J_1(2x) = \sum_{k=0}^\infty \frac{(-1)^k}{k! \, \Gamma(k+2)} x^{2k+1}
\]

So,
\[
I = \int_0^1 \arccos x \, J_1(2x) \, dx = \sum_{k=0}^\infty \frac{(-1)^k 2^{2k+1}}{k! \, \Gamma(k+2)} \int_0^1 \arccos x \, x^{2k+1} dx
\]

Let’s compute the inner integral:
\[
I_k = \int_0^1 \arccos x \, x^{2k+1} dx
\]

Let’s use the substitution \( x = \cos\theta \), \( dx = -\sin\theta d\theta \), as before.

When \( x = 0 \), \( \theta = \frac{\pi}{2} \), when \( x = 1 \), \( \theta = 0 \).

So,
\[
I_k = \int_{x=0}^{x=1} \arccos x \, x^{2k+1} dx = \int_{\theta=\frac{\pi}{2}}^{\theta=0} \theta \cos^{2k+1}\theta \, (-\sin\theta) d\theta
\]
\[
= \int_{0}^{\frac{\pi}{2}} \theta \cos^{2k+1}\theta \sin\theta d\theta
\]

Let’s write \( \cos^{2k+1}\theta \sin\theta = \frac{1}{2k+2} \frac{d}{d\theta}(-\cos^{2k+2}\theta) \):

Let’s use integration by parts:

Let \( u = \theta \), \( dv = \cos^{2k+1}\theta \sin\theta d\theta \).

Then \( du = d\theta \), \( v = -\frac{1}{2k+2} \cos^{2k+2}\theta \).

So,
\[
I_k = u v \Big|_0^{\frac{\pi}{2}} - \int_0^{\frac{\pi}{2}} v du
\]
\[
= \left. -\frac{\theta}{2k+2} \cos^{2k+2}\theta \right|_0^{\frac{\pi}{2}} + \int_0^{\frac{\pi}{2}} \frac{1}{2k+2} \cos^{2k+2}\theta d\theta
\]

But at \( \theta = 0 \), \( \cos 0 = 1 \), so \( \cos^{2k+2} 0 = 1 \), at \( \theta = \frac{\pi}{2} \), \( \cos \frac{\pi}{2} = 0 \), so \( \cos^{2k+2} \frac{\pi}{2} = 0 \).

So,
\[
I_k = -\frac{0}{2k+2} \cdot 0 + \frac{1}{2k+2} \cdot 1 - \int_0^{\frac{\pi}{2}} \frac{1}{2k+2} \cos^{2k+2}\theta d\theta
\]
Wait, the boundary term is:
\[
-\frac{\theta}{2k+2} \cos^{2k+2}\theta \Big|_0^{\frac{\pi}{2}} = -\frac{\frac{\pi}{2}}{2k+2} \cdot 0 + \frac{0}{2k+2} \cdot 1 = 0
\]
So the boundary term is zero.

So,
\[
I_k = \frac{1}{2k+2} \int_0^{\frac{\pi}{2}} \cos^{2k+2}\theta d\theta
\]

But this is a standard integral:
\[
\int_0^{\frac{\pi}{2}} \cos^n\theta d\theta = \frac{\sqrt{\pi} \, \Gamma\left(\frac{n+1}{2}\right)}{2 \, \Gamma\left(\frac{n}{2} + 1\right)}
\]
So for \( n = 2k+2 \):
\[
I_k = \frac{1}{2k+2} \cdot \frac{\sqrt{\pi} \, \Gamma\left(k+\frac{3}{2}\right)}{2 \, \Gamma(k+2)}
\]

**Step 3: Substitute back into the sum**

Recall:
\[
I = \sum_{k=0}^\infty \frac{(-1)^k 2^{2k+1}}{k! \, \Gamma(k+2)} I_k
\]
\[
= \sum_{k=0}^\infty \frac{(-1)^k 2^{2k+1}}{k! \, \Gamma(k+2)} \cdot \frac{1}{2k+2} \cdot \frac{\sqrt{\pi} \, \Gamma\left(k+\frac{3}{2}\right)}{2 \, \Gamma(k+2)}
\]
\[
= \sum_{k=0}^\infty \frac{(-1)^k 2^{2k+1} \sqrt{\pi} \, \Gamma\left(k+\frac{3}{2}\right)}{k! \, (2k+2) \cdot 2 \, [\Gamma(k+2)]^2}
\]
\[
= \sum_{k=0}^\infty \frac{(-1)^k 2^{2k} \sqrt{\pi} \, \Gamma\left(k+\frac{3}{2}\right)}{k! \, (k+1) \, [\Gamma(k+2)]^2}
\]

**Step 4: Try to find a closed form**

Alternatively, let's try to find a closed form by integrating by parts the original integral.

Let’s try integrating by parts in the original variable:

Let \( u = \arccos x \), \( dv = J_1(2x) dx \), so \( du = -\frac{1}{\sqrt{1-x^2}} dx \), \( v = \int J_1(2x) dx \).

But \( \int J_1(2x) dx = -J_0(2x)/2 + C \).

So,
\[
I = \left. \arccos x \cdot \left(-\frac{1}{2} J_0(2x)\right) \right|_0^1 - \int_0^1 \left(-\frac{1}{2} J_0(2x)\right) \cdot \left(-\frac{1}{\sqrt{1-x^2}}\right) dx
\]
\[
= -\frac{1}{2} \left[ \arccos x \cdot J_0(2x) \right]_0^1 - \frac{1}{2} \int_0^1 \frac{J_0(2x)}{\sqrt{1-x^2}} dx
\]

Now, evaluate the boundary term:

- At \( x = 1 \): \( \arccos 1 = 0 \), \( J_0(2 \cdot 1) = J_0(2) \), so the term is 0.
- At \( x = 0 \): \( \arccos 0 = \frac{\pi}{2} \), \( J_0(0) = 1 \), so the term is \( \frac{\pi}{2} \cdot 1 \).

So,
\[
\left[ \arccos x \cdot J_0(2x) \right]_0^1 = 0 - \frac{\pi}{2} \cdot 1 = -\frac{\pi}{2}
\]

So,
\[
I = -\frac{1}{2} \left(-\frac{\pi}{2}\right) - \frac{1}{2} \int_0^1 \frac{J_0(2x)}{\sqrt{1-x^2}} dx
\]
\[
= \frac{\pi}{4} - \frac{1}{2} \int_0^1 \frac{J_0(2x)}{\sqrt{1-x^2}} dx
\]

Now, the remaining integral is a standard one:

\[
\int_0^1 \frac{J_0(2x)}{\sqrt{1-x^2}} dx
\]

Let’s use the substitution \( x = \sin\theta \), \( dx = \cos\theta d\theta \), as \( x \) goes from 0 to 1, \( \theta \) goes from 0 to \( \frac{\pi}{2} \):

- \( \sqrt{1-x^2} = \cos\theta \)
- \( J_0(2x) = J_0(2\sin\theta) \)
- \( dx = \cos\theta d\theta \)

So,
\[
\int_0^1 \frac{J_0(2x)}{\sqrt{1-x^2}} dx = \int_{\theta=0}^{\theta=\frac{\pi}{2}} \frac{J_0(2\sin\theta)}{\cos\theta} \cdot \cos\theta d\theta = \int_0^{\frac{\pi}{2}} J_0(2\sin\theta) d\theta
\]

But this is a standard integral (see Gradshteyn & Ryzhik 6.671.7):

\[
\int_0^{\pi/2} J_0(a \sin\theta) d\theta = \frac{\pi}{2} J_0(a/2)
\]
But for \( a = 2 \):

\[
\int_0^{\pi/2} J_0(2\sin\theta) d\theta = \frac{\pi}{2} J_0(1)
\]

Therefore,
\[
I = \frac{\pi}{4} - \frac{1}{2} \cdot \frac{\pi}{2} J_0(1) = \frac{\pi}{4} - \frac{\pi}{4} J_0(1) = \frac{\pi}{4} (1 - J_0(1))
\]

**Step 5: Numerical Approximation**

\( J_0(1) \approx 0.7651976866 \)

So,
\[
I \approx \frac{\pi}{4} (1 - 0.7651976866) = \frac{\pi}{4} \cdot 0.2348023134 \approx 0.1844530406
\]

**Final Answer in JSON Format**

```json
{"answer": "\\frac{\\pi}{4} \\left(1 - J_0(1)\\right)", "numerical_answer": "0.1844530406"}
```