Let's proceed step by step.

**Step 1: Identify \( H_3 \)**
The third Hermite polynomial is:
\[
H_3(x) = 8x^3 - 12x
\]

**Step 2: Plug in to the integral**
The definite integral is:
\[
I = \int_0^2 H_3\big(\sqrt{x(2-x)}\big) \, dx
\]
\[
= \int_0^2 \left[ 8\left(\sqrt{x(2-x)}\right)^3 - 12\sqrt{x(2-x)} \right] dx
\]
Let’s simplify \( \left(\sqrt{x(2-x)}\right)^3 = \left(x(2-x)\right)^{3/2} \)
So:
\[
I = 8\int_0^2 [x(2-x)]^{3/2} dx - 12\int_0^2 [x(2-x)]^{1/2} dx
\]

Let \( I_1 = \int_0^2 [x(2-x)]^{3/2} dx \), \( I_2 = \int_0^2 [x(2-x)]^{1/2} dx \). Then \( I = 8I_1 - 12I_2 \).

**Step 3: Compute \( I_1 \) and \( I_2 \) via substitution**

Let’s use the substitution \( x = 2\sin^2\theta \), so that \( 0 \leq x \leq 2 \) maps to \( 0 \leq \theta \leq \pi/2 \).
Then:
- \( dx = 4\sin\theta\cos\theta\, d\theta = 2\sin2\theta\, d\theta \)
- \( x(2-x) = 2\sin^2\theta(2-2\sin^2\theta) = 4\sin^2\theta\cos^2\theta = \sin^2 2\theta \)

So:

\[
I_n = \int_0^2 [x(2-x)]^{n/2} dx = \int_{0}^{\pi/2} [\sin^2 2\theta]^{n/2} \cdot 2\sin2\theta\, d\theta
\]
\[
= 2\int_0^{\pi/2} \sin^n 2\theta \cdot \sin2\theta\, d\theta = 2\int_0^{\pi/2} \sin^{n+1} 2\theta\, d\theta
\]

Let’s perform the substitution \( u = 2\theta \), then when \( \theta = 0 \), \( u = 0 \); \( \theta = \pi/2 \), \( u = \pi \); \( d\theta = du/2 \):

\[
I_n = 2\int_{\theta=0}^{\theta=\pi/2} \sin^{n+1} 2\theta\, d\theta = 2 \cdot \int_{u=0}^{u=\pi} \sin^{n+1}u \cdot \frac{du}{2}
= \int_0^\pi \sin^{n+1} u \, du
\]

Therefore:

\[
I_1 = \int_0^\pi \sin^{4} u \, du
\]
\[
I_2 = \int_0^\pi \sin^{2} u \, du
\]

And so:
\[
I = 8I_1 - 12I_2 = 8 \int_0^\pi \sin^4 u\, du - 12 \int_0^\pi \sin^2 u\, du
\]

**Step 4: Compute \( \int_0^\pi \sin^2 u\, du \) and \( \int_0^\pi \sin^4 u\, du \) **

Recall:

- \( \int_0^\pi \sin^2u\, du = \frac{\pi}{2} \)
- \( \int_0^\pi \sin^4u\, du = \frac{3\pi}{8} \)

(see, e.g., standard integrals or use the reduction formula/integral.)

**Derivation: For completeness:**

\[
\sin^2u = \frac{1}{2}(1 - \cos 2u)
\]
So
\[
\int_0^\pi \sin^2u\, du = \frac{1}{2} \int_0^\pi 1\, du - \frac{1}{2}\int_0^\pi \cos 2u\, du
= \frac{\pi}{2} - \frac{1}{2} \cdot 0 = \frac{\pi}{2}
\]

Now, for \( \sin^4 u \):

\[
\sin^4 u = \left(\sin^2 u\right)^2 = \left(\frac{1 - \cos 2u}{2}\right)^2
= \frac{1}{4}\left(1 - 2\cos 2u + \cos^2 2u\right)
\]

But \( \cos^2 2u = \frac{1 + \cos 4u}{2} \):

Thus,
\[
\sin^4 u = \frac{1}{4}\left(1 - 2\cos2u + \frac{1+\cos4u}{2}\right)
= \frac{1}{4}(1 - 2\cos2u) + \frac{1}{8}(1 + \cos4u)
= \frac{1}{4} - \frac{1}{2}\cos2u + \frac{1}{8} + \frac{1}{8}\cos4u
= \frac{3}{8} - \frac{1}{2}\cos2u + \frac{1}{8}\cos4u
\]

Therefore:
\[
\int_0^\pi \sin^4 u\, du = \frac{3}{8}\pi - \frac{1}{2}\int_0^\pi \cos2u\, du + \frac{1}{8}\int_0^\pi \cos4u\, du
\]
But \( \int_0^\pi \cos2u\, du = 0 \), \( \int_0^\pi \cos4u\, du = 0 \). So:
\[
\int_0^\pi \sin^4 u\, du = \frac{3}{8}\pi
\]

**Step 5: Plug in values**
\[
I = 8\cdot\frac{3}{8}\pi - 12\cdot\frac{\pi}{2} = 3\pi - 6\pi = -3\pi
\]

**Step 6: Numerical answer to 10 decimal places**

\[
-3\pi \approx -3 \times 3.1415926536 = -9.4247779608
\]

**Final JSON output:**
```json
{"answer": "-3\\pi", "numerical_answer": "-9.4247779608"}
```