
To solve the definite integral \( \int_0^{2} x^{-1/4} (2 - x)^{-3/4} I_1\left( \sqrt[4]{x(2 - x)} \right) dx \), we proceed as follows:


### Step 1: Substitution to Simplify the Integral
Let \( x = 2u \), so \( dx = 2du \). When \( x = 0 \), \( u = 0 \); when \( x = 2 \), \( u = 1 \). Substituting \( x = 2u \) transforms the integral:
\[
\begin{aligned}
x^{-1/4} &= (2u)^{-1/4} = 2^{-1/4} u^{-1/4}, \\
(2 - x)^{-3/4} &= (2(1 - u))^{-3/4} = 2^{-3/4} (1 - u)^{-3/4}, \\
\sqrt[4]{x(2 - x)} &= \sqrt[4]{2u \cdot 2(1 - u)} = \sqrt[4]{4u(1 - u)} = \sqrt{2} \cdot \sqrt[4]{u(1 - u)}.
\end{aligned}
\]
The integral becomes:
\[
\int_0^1 2^{-1/4} u^{-1/4} \cdot 2^{-3/4} (1 - u)^{-3/4} \cdot I_1\left( \sqrt{2} \cdot \sqrt[4]{u(1 - u)} \right) \cdot 2 \, du.
\]
Simplifying constants: \( 2^{-1/4 - 3/4} \cdot 2 = 2^{-1} \cdot 2 = 1 \). Thus:
\[
\int_0^1 u^{-1/4} (1 - u)^{-3/4} I_1\left( \sqrt{2} \cdot \sqrt[4]{u(1 - u)} \right) du.
\]


### Step 2: Series Expansion of the Bessel Function
The modified Bessel function \( I_1(z) \) has the series expansion:
\[
I_1(z) = \sum_{k=0}^\infty \frac{(z/2)^{1 + 2k}}{k! (k + 1)!}.
\]
Substituting \( z = \sqrt{2} \cdot \sqrt[4]{u(1 - u)} \), we get:
\[
I_1\left( \sqrt{2} \cdot \sqrt[4]{u(1 - u)} \right) = \sum_{k=0}^\infty \frac{\left( \sqrt{2} \cdot \sqrt[4]{u(1 - u)} / 2 \right)^{1 + 2k}}{k! (k + 1)!}.
\]
Simplifying the argument:
\[
\left( \sqrt{2} \cdot \sqrt[4]{u(1 - u)} / 2 \right)^{1 + 2k} = 2^{(1 + 2k)/2 - (1 + 2k)} \cdot u^{(1 + 2k)/4} (1 - u)^{(1 + 2k)/4} = 2^{-(1 + 2k)/2} \cdot u^{(1 + 2k)/4} (1 - u)^{(1 + 2k)/4}.
\]


### Step 3: Interchange Summation and Integration
Substituting the series into the integral and interchanging summation and integration (justified by uniform convergence):
\[
\int_0^1 u^{-1/4} (1 - u)^{-3/4} \sum_{k=0}^\infty \frac{2^{-(1 + 2k)/2} \cdot u^{(1 + 2k)/4} (1 - u)^{(1 + 2k)/4}}{k! (k + 1)!} du.
\]
Simplifying the exponents of \( u \) and \( (1 - u) \):
\[
u^{-1/4 + (1 + 2k)/4} = u^{k/2}, \quad (1 - u)^{-3/4 + (1 + 2k)/4} = (1 - u)^{(k - 1)/2}.
\]
The integral reduces to a Beta function:
\[
\int_0^1 u^{k/2} (1 - u)^{(k - 1)/2} du = B\left( \frac{k}{2} + 1, \frac{k - 1}{2} + 1 \right) = \frac{\Gamma\left( \frac{k + 2}{2} \right) \Gamma\left( \frac{k + 1}{2} \right)}{\Gamma\left( \frac{2k + 3}{2} \right)}.
\]


### Step 4: Simplifying the Beta Function
Using properties of the Gamma function (e.g., duplication formula), the Beta function simplifies to:
\[
B\left( \frac{k + 2}{2}, \frac{k + 1}{2} \right) = \frac{2^{k + 1} (k!)^2}{(2k + 1)!}.
\]
Substituting back, the integral becomes:
\[
\sum_{k=0}^\infty \frac{\sqrt{2}}{(k + 1) (2k + 1)!}.
\]


### Step 5: Evaluating the Series
The series \( \sum_{m=1}^\infty \frac{1}{m (2m - 1)!} \) is recognized as \( 2(\cosh(1) - 1) \) (by integrating the series expansion of \( \sinh(z) \)). Thus:
\[
\int_0^2 x^{-1/4} (2 - x)^{-3/4} I_1\left( \sqrt[4]{x(2 - x)} \right) dx = 2\sqrt{2} (\cosh(1) - 1).
\]


### Numerical Approximation
Using \( \cosh(1) = \frac{e + 1/e}{2} \approx 1.5430806348 \), we find:
\[
2\sqrt{2} (\cosh(1) - 1) \approx 2\sqrt{2} (0.5430806348) \approx 1.536064340.
\]


### Final Answer
{"answer": "2\\sqrt{2} (\\cosh(1) - 1)", "numerical_answer": "1.5360643400"}