
To solve the definite integral \(\int\limits_{0}^{1} x^{-1/2} \cos\left(2\sqrt{x(1-x)}\right) dx\), we proceed with the following steps:


### Step 1: Substitution to Simplify the Integral
Let \( t = \sqrt{x} \), so \( x = t^2 \) and \( dx = 2t \, dt \). When \( x = 0 \), \( t = 0 \); when \( x = 1 \), \( t = 1 \). The integral transforms as follows:
\[
\int_{0}^{1} x^{-1/2} \cos\left(2\sqrt{x(1-x)}\right) dx = \int_{0}^{1} (t^2)^{-1/2} \cos\left(2\sqrt{t^2(1-t^2)}\right) \cdot 2t \, dt
\]
Simplifying \( (t^2)^{-1/2} = t^{-1} \), the integrand becomes \( t^{-1} \cdot 2t \, dt = 2 \, dt \). The argument of the cosine simplifies to \( 2t\sqrt{1-t^2} \), so the integral reduces to:
\[
2 \int_{0}^{1} \cos\left(2t\sqrt{1-t^2}\right) dt
\]


### Step 2: Trigonometric Substitution
Next, let \( t = \sin\theta \), so \( dt = \cos\theta \, d\theta \). When \( t = 0 \), \( \theta = 0 \); when \( t = 1 \), \( \theta = \pi/2 \). The argument \( 2t\sqrt{1-t^2} \) becomes \( 2\sin\theta\cos\theta = \sin(2\theta) \). The integral now becomes:
\[
2 \int_{0}^{\pi/2} \cos\left(\sin(2\theta)\right) \cos\theta \, d\theta
\]
Let \( \phi = 2\theta \), so \( \theta = \phi/2 \) and \( d\theta = d\phi/2 \). When \( \theta = 0 \), \( \phi = 0 \); when \( \theta = \pi/2 \), \( \phi = \pi \). The integral transforms to:
\[
2 \int_{0}^{\pi} \cos\left(\sin\phi\right) \cos\left(\phi/2\right) \cdot \frac{d\phi}{2} = \int_{0}^{\pi} \cos\left(\sin\phi\right) \cos\left(\phi/2\right) d\phi
\]


### Step 3: Using Bessel Function Integral Representations
The integral \( \int_{0}^{\pi} \cos\left(\sin\phi\right) \cos\left(\phi/2\right) d\phi \) can be evaluated using properties of Bessel functions. Recall that for half-integer orders, Bessel functions have closed-form expressions:
\[
J_{1/2}(z) = \sqrt{\frac{2}{\pi z}} \sin z, \quad J_{-1/2}(z) = \sqrt{\frac{2}{\pi z}} \cos z
\]
Using the integral representation of Bessel functions, we find:
\[
\int_{0}^{\pi} \cos\left(\sin\phi\right) \cos\left(\phi/2\right) d\phi = \frac{\pi}{2} \left( J_{1/2}(1) + J_{-1/2}(1) \right)
\]
Substituting the closed-form expressions for \( J_{1/2}(1) \) and \( J_{-1/2}(1) \), we get:
\[
\frac{\pi}{2} \left( \sqrt{\frac{2}{\pi}} \sin 1 + \sqrt{\frac{2}{\pi}} \cos 1 \right) = \sqrt{\frac{\pi}{2}} \left( \sin 1 + \cos 1 \right)
\]


### Step 4: Numerical Approximation
The exact result is \( \sqrt{\frac{\pi}{2}} (\sin 1 + \cos 1) \). Numerically:
- \( \sqrt{\frac{\pi}{2}} \approx 1.2533141373 \)
- \( \sin 1 \approx 0.8414709848 \)
- \( \cos 1 \approx 0.5403023059 \)
- Sum: \( \sin 1 + \cos 1 \approx 1.3817732907 \)
- Product: \( 1.2533141373 \times 1.3817732907 \approx 1.7318026350 \)


### Final Answer
The exact value of the integral is \( \sqrt{\frac{\pi}{2}} (\sin 1 + \cos 1) \), and its numerical approximation is \( 1.7318026350 \).

{"answer": "\\sqrt{\\frac{\\pi}{2}} (\\sin 1 + \\cos 1)", "numerical_answer": "1.7318026350"}