Let's compute the definite integral:

\[
\int_{-1}^1 (5x^3 - 3x)^2\,dx
\]

**Step 1: Expand the Integrand**

\[
(5x^3 - 3x)^2 = (5x^3)^2 - 2 \cdot 5x^3 \cdot 3x + (3x)^2 = 25x^6 - 30x^4 + 9x^2
\]

**Step 2: Write the Integral with Expanded Terms**

\[
\int_{-1}^1 (25x^6 - 30x^4 + 9x^2)\,dx = 25\int_{-1}^1 x^6\,dx - 30\int_{-1}^1 x^4\,dx + 9\int_{-1}^1 x^2\,dx
\]

**Step 3: Compute Each Integral Individually**

The antiderivative of \(x^n\) is \(\frac{x^{n+1}}{n+1}\).

- \(\int_{-1}^1 x^6\,dx = \left[\frac{x^7}{7}\right]_{-1}^1 = \frac{1^7}{7} - \frac{(-1)^7}{7} = \frac{1}{7} - \left(-\frac{1}{7}\right) = \frac{2}{7}\)
- \(\int_{-1}^1 x^4\,dx = \left[\frac{x^5}{5}\right]_{-1}^1 = \frac{1^5}{5} - \frac{(-1)^5}{5} = \frac{1}{5} - \left(-\frac{1}{5}\right) = \frac{2}{5}\)
- \(\int_{-1}^1 x^2\,dx = \left[\frac{x^3}{3}\right]_{-1}^1 = \frac{1^3}{3} - \frac{(-1)^3}{3} = \frac{1}{3} - \left(-\frac{1}{3}\right) = \frac{2}{3}\)

**Step 4: Substitute Back and Simplify**

\[
= 25 \cdot \frac{2}{7} - 30 \cdot \frac{2}{5} + 9 \cdot \frac{2}{3}
\]
\[
= \frac{50}{7} - \frac{60}{5} + \frac{18}{3}
\]
\[
= \frac{50}{7} - 12 + 6
\]
\[
= \frac{50}{7} - 6
\]
\[
= \frac{50 - 42}{7}
\]
\[
= \frac{8}{7}
\]

**Step 5: Numerical Approximation**

\[
\frac{8}{7} \approx 1.1428571429
\]

**Final JSON Output:**

```json
{"answer": "\\frac{8}{7}", "numerical_answer": "1.1428571429"}
```