<think>
Okay, let's tackle this integral step by step. The integral given is ∫₀² x^(-1/2) [1 + 1.0√(x(2.0 - x))]^(-3/2) dx. Hmm, first, I need to see if there's a substitution that can simplify this expression. The presence of √(x(2 - x)) suggests maybe a trigonometric substitution or something that can exploit the symmetry of the expression under the square root.

Let me consider the variable substitution. The term x(2 - x) is a quadratic that can be rewritten as 2x - x², which is similar to the form of 1 - (x - 1)². Wait, if I complete the square here: 2x - x² = -(x² - 2x) = -(x² - 2x +1 -1) = -(x -1)^2 +1. So, √(x(2 -x)) = √[1 - (x -1)^2]. That looks like the equation of a semicircle with radius 1 centered at (1,0). So maybe a trigonometric substitution where x -1 = sinθ? Let's try that.

Let’s set x = 1 + sinθ. Then, dx = cosθ dθ. But we need to adjust the limits of integration. When x=0, 0 = 1 + sinθ ⇒ sinθ = -1 ⇒ θ = -π/2. When x=2, 2 =1 + sinθ ⇒ sinθ =1 ⇒ θ=π/2. So the new limits are from -π/2 to π/2. Let's substitute into the integral.

First, x^(-1/2) becomes (1 + sinθ)^(-1/2). The term √(x(2 -x)) becomes √[1 - (x -1)^2] = √[1 - sin²θ] = cosθ. So the denominator becomes [1 + 1.0 * cosθ]^(-3/2) = [1 + cosθ]^(-3/2). Therefore, the integral becomes:

∫ from θ=-π/2 to θ=π/2 of (1 + sinθ)^(-1/2) * [1 + cosθ]^(-3/2) * cosθ dθ.

Hmm, that seems a bit complicated. Let me check if I did the substitution correctly. Wait, the original integrand is x^(-1/2) times [1 + sqrt(x(2 -x))]^(-3/2). After substitution, x is 1 + sinθ, so x^(-1/2) is (1 + sinθ)^(-1/2). The sqrt(x(2 -x)) is sqrt(1 - (x-1)^2) which is cosθ, so the denominator becomes (1 + cosθ)^(3/2). Then, dx is cosθ dθ. So the integrand is (1 + sinθ)^(-1/2) * (1 + cosθ)^(-3/2) * cosθ dθ. That's correct.

But this still looks tricky. Maybe there's a way to simplify the expression (1 + sinθ)^(-1/2) * (1 + cosθ)^(-3/2). Let's recall some trigonometric identities. 1 + cosθ can be written as 2 cos²(θ/2), and 1 + sinθ can be written as 2 sin²(θ/2 + π/4) or something similar. Let me check:

1 + sinθ = 2 sin²(θ/2 + π/4) + ... Wait, actually, 1 + sinθ = 2 sin²(θ/2 + π/4) is not correct. Let me recall the identity: sinθ = 2 sin(θ/2) cos(θ/2), and 1 + sinθ = (sin(θ/2) + cos(θ/2))². Let's verify:

(sin(θ/2) + cos(θ/2))² = sin²(θ/2) + 2 sin(θ/2)cos(θ/2) + cos²(θ/2) = 1 + sinθ. Yes, that's correct. So 1 + sinθ = (sin(θ/2) + cos(θ/2))². Similarly, 1 + cosθ = 2 cos²(θ/2).

So substituting these into the integrand:

(1 + sinθ)^(-1/2) = [ (sin(θ/2) + cos(θ/2))² ]^(-1/2) = 1 / (sin(θ/2) + cos(θ/2)).

(1 + cosθ)^(-3/2) = [2 cos²(θ/2)]^(-3/2) = 2^(-3/2) * cos^(-3)(θ/2).

So putting it all together, the integrand becomes:

[1 / (sin(θ/2) + cos(θ/2))] * [2^(-3/2) cos^(-3)(θ/2)] * cosθ dθ.

Wait, and the cosθ term from dx is still there. Let's also express cosθ in terms of θ/2. cosθ = 2 cos²(θ/2) -1. Hmm, but maybe there's a better way. Let's substitute all the terms step by step.

First, let's write the entire integrand:

(1 + sinθ)^(-1/2) * (1 + cosθ)^(-3/2) * cosθ dθ

= [ (sin(θ/2) + cos(θ/2))² ]^(-1/2) * [2 cos²(θ/2)]^(-3/2) * cosθ dθ

= [1/(sin(θ/2) + cos(θ/2))] * [2^(-3/2) cos^{-3}(θ/2)] * cosθ dθ

Now, cosθ can be written as 2 cos²(θ/2) -1. But maybe that's not helpful. Alternatively, let's express cosθ in terms of θ/2:

cosθ = 1 - 2 sin²(θ/2) = 2 cos²(θ/2) -1. Hmm. Alternatively, perhaps we can make another substitution here. Let me see.

Alternatively, let's consider substituting t = θ/2. Then θ = 2t, dθ = 2dt. The limits when θ is from -π/2 to π/2, t is from -π/4 to π/4.

But maybe that's not the way. Alternatively, let's try to manipulate the integrand:

Let me write the integrand as:

[1/(sin(θ/2) + cos(θ/2))] * [2^{-3/2} cos^{-3}(θ/2)] * cosθ * dθ

Let me factor out the constants:

2^{-3/2} * [1/(sin(θ/2) + cos(θ/2))] * [cos^{-3}(θ/2)] * cosθ * dθ

Now, let's express cosθ in terms of θ/2:

cosθ = 2 cos²(θ/2) -1. So:

= 2^{-3/2} * [1/(sin(θ/2) + cos(θ/2))] * [cos^{-3}(θ/2)] * [2 cos²(θ/2) -1] * dθ

Hmm, this seems messy. Maybe there's a better substitution. Let's think again.

Alternatively, perhaps a substitution u = θ/2 + π/4. Let me see. Let's try to rationalize the denominator sin(θ/2) + cos(θ/2). Let's factor out cos(θ/2):

sin(θ/2) + cos(θ/2) = cos(θ/2)[1 + tan(θ/2)]

But not sure. Alternatively, we can write sin(θ/2) + cos(θ/2) = √2 sin(θ/2 + π/4). Let's check:

√2 sin(θ/2 + π/4) = √2 [sin(θ/2) cos(π/4) + cos(θ/2) sin(π/4)] = √2 [ (sin(θ/2) + cos(θ/2)) / √2 ] = sin(θ/2) + cos(θ/2). Yes, that's correct. So sin(θ/2) + cos(θ/2) = √2 sin(θ/2 + π/4). Therefore, 1/(sin(θ/2) + cos(θ/2)) = 1/(√2 sin(θ/2 + π/4)).

So substituting back into the integrand:

2^{-3/2} * [1/(√2 sin(θ/2 + π/4))] * [cos^{-3}(θ/2)] * cosθ dθ

= 2^{-3/2 -1/2} * [1/sin(θ/2 + π/4)] * [cos^{-3}(θ/2)] * cosθ dθ

= 2^{-2} * [1/sin(θ/2 + π/4)] * [cos^{-3}(θ/2)] * cosθ dθ

= (1/4) * [1/sin(θ/2 + π/4)] * [cos^{-3}(θ/2)] * cosθ dθ

Hmm, still complicated. Maybe another substitution. Let's set t = θ/2 + π/4. Then θ = 2(t - π/4), dθ = 2dt. When θ = -π/2, t = (-π/2)/2 + π/4 = -π/4 + π/4 = 0. Wait, no:

Wait, θ ranges from -π/2 to π/2. So θ = -π/2: t = (-π/2)/2 + π/4 = -π/4 + π/4 = 0. θ = π/2: t = (π/2)/2 + π/4 = π/4 + π/4 = π/2. So the new limits are from t=0 to t=π/2. Wait, but when θ=-π/2, t= (-π/2)/2 + π/4 = -π/4 + π/4 = 0. When θ=π/2, t= (π/2)/2 + π/4 = π/4 + π/4 = π/2. So the substitution t = θ/2 + π/4 changes the limits to 0 to π/2. Let's proceed.

So θ = 2(t - π/4), dθ = 2dt. Let's express all terms in terms of t.

First, sin(θ/2 + π/4) = sin(t). Because θ/2 + π/4 = t. So 1/sin(θ/2 + π/4) = 1/sin t.

Next, cos(θ/2) = cos(t - π/4). Because θ/2 = t - π/4. So cos(θ/2) = cos(t - π/4) = cos t cos π/4 + sin t sin π/4 = (cos t + sin t)/√2.

Similarly, cosθ = cos[2(t - π/4)] = cos(2t - π/2) = cos(2t)cos(π/2) + sin(2t)sin(π/2) = sin(2t).

So substituting all these:

The integrand becomes:

(1/4) * [1/sin t] * [ ( (cos t + sin t)/√2 )^{-3} ] * sin(2t) * 2 dt

Let's simplify step by step.

First, sin(2t) = 2 sin t cos t. So:

= (1/4) * [1/sin t] * [ ( (cos t + sin t)/√2 )^{-3} ] * 2 sin t cos t * 2 dt

Wait, the 2 comes from dθ = 2dt. Wait, no: the original integrand after substitution includes dθ = 2dt. Wait, let's re-express the entire substitution:

Original integrand after substitution:

(1/4) * [1/sin t] * [ ( (cos t + sin t)/√2 )^{-3} ] * sin(2t) * 2 dt

Wait, let's check each part:

- The 1/4 comes from 2^{-2} (earlier steps)
- The [1/sin t] comes from 1/sin(θ/2 + π/4) = 1/sin t
- [ (cos t + sin t)/√2 )^{-3} ] comes from [cos(θ/2)]^{-3} = [ (cos t + sin t)/√2 ]^{-3}
- cosθ = sin(2t)
- dθ = 2 dt

Wait, but in the substitution, the integrand had a cosθ dθ term. Wait, let's retrace:

Original integrand after substitution was:

(1/4) * [1/sin t] * [ ( (cos t + sin t)/√2 )^{-3} ] * sin(2t) * 2 dt

Wait, perhaps I made a miscalculation here. Let me re-express:

After substitution t = θ/2 + π/4, θ = 2(t - π/4), dθ = 2 dt.

So the integrand becomes:

(1/4) * [1/sin t] * [ ( (cos t + sin t)/√2 )^{-3} ] * cosθ * 2 dt

But cosθ = sin(2t), as we had earlier. So cosθ = sin(2t). Therefore:

= (1/4) * [1/sin t] * [ ( (cos t + sin t)/√2 )^{-3} ] * sin(2t) * 2 dt

Now, sin(2t) = 2 sin t cos t. So substituting that:

= (1/4) * [1/sin t] * [ ( (cos t + sin t)/√2 )^{-3} ] * 2 sin t cos t * 2 dt

The 2 from sin(2t) and the 2 from dθ multiply to give 4. Wait, let's compute step by step:

First, the constants:

(1/4) * 2 (from dθ) = (1/4)*2 = 1/2

Then, the terms:

[1/sin t] * [ ( (cos t + sin t)/√2 )^{-3} ] * sin(2t) 

= [1/sin t] * [ (cos t + sin t)^{-3} / (2^{-3/2}) ] * 2 sin t cos t

= [1/sin t] * [2^{3/2} / (cos t + sin t)^3 ] * 2 sin t cos t

= 2^{3/2} * 2 * [1/sin t] * sin t * cos t / (cos t + sin t)^3

= 2^{5/2} * cos t / (cos t + sin t)^3

So combining with the constants:

1/2 * 2^{5/2} * cos t / (cos t + sin t)^3 dt

= (2^{5/2} / 2) ) * cos t / (cos t + sin t)^3 dt

= 2^{3/2} * cos t / (cos t + sin t)^3 dt

Hmm, so the integral becomes:

2^{3/2} ∫ from t=0 to t=π/2 [cos t / (cos t + sin t)^3] dt

This seems more manageable. Let's see if we can simplify this integral. Let's consider the denominator (cos t + sin t)^3. Maybe a substitution u = tan t, but let's see.

Alternatively, let's note that cos t + sin t = √2 sin(t + π/4). But perhaps another substitution. Let's set u = tan t. Then t goes from 0 to π/2, so u goes from 0 to ∞. But integrating from 0 to ∞ might be challenging. Alternatively, let's split the integral into two parts or use symmetry.

Alternatively, let's make substitution s = π/2 - t. When t=0, s=π/2; when t=π/2, s=0. So the integral becomes:

2^{3/2} ∫ from s=π/2 to s=0 [cos(π/2 - s) / (cos(π/2 - s) + sin(π/2 - s))^3 ] (-ds)

= 2^{3/2} ∫ from s=0 to s=π/2 [sin s / (sin s + cos s)^3 ] ds

But this is the same as the original integral with cos t replaced by sin s. So adding the original integral and this one:

Original integral: I = 2^{3/2} ∫₀^{π/2} [cos t / (cos t + sin t)^3 ] dt

After substitution, we have I = 2^{3/2} ∫₀^{π/2} [sin t / (sin t + cos t)^3 ] dt

So adding them: 2I = 2^{3/2} ∫₀^{π/2} [ (cos t + sin t) / (cos t + sin t)^3 ] dt = 2^{3/2} ∫₀^{π/2} [1 / (cos t + sin t)^2 ] dt

Thus, 2I = 2^{3/2} ∫₀^{π/2} [1 / (cos t + sin t)^2 ] dt

But cos t + sin t = √2 sin(t + π/4), so (cos t + sin t)^2 = 2 sin²(t + π/4). Therefore:

2I = 2^{3/2} ∫₀^{π/2} [1 / (2 sin²(t + π/4)) ] dt = 2^{3/2} * (1/2) ∫₀^{π/2} csc²(t + π/4) dt

= 2^{1/2} ∫₀^{π/2} csc²(t + π/4) dt

The integral of csc²(u) du is -cot(u) + C. So:

= 2^{1/2} [ -cot(t + π/4) ] from t=0 to t=π/2

= 2^{1/2} [ -cot(π/2 + π/4) + cot(0 + π/4) ]

cot(3π/4) = -1, and cot(π/4) = 1. So:

= 2^{1/2} [ -(-1) + 1 ] = 2^{1/2} [1 +1] = 2^{1/2} * 2 = 2^{3/2}

Therefore, 2I = 2^{3/2} ⇒ I = 2^{3/2}/2 = 2^{1/2} = √2

Wait, so the integral I is √2. Therefore, the original integral, which after substitution became I = √2, but wait, let's check:

Wait, the original integral after substitution was:

I = 2^{3/2} ∫₀^{π/2} [cos t / (cos t + sin t)^3 ] dt

But we found that 2I = 2^{3/2} * (something) which led to 2I = 2^{3/2} * (√2) ?

Wait, no, let's retrace:

Wait, after substitution, we had:

Original integral after substitution was I = 2^{3/2} ∫₀^{π/2} [cos t / (cos t + sin t)^3 ] dt

Then, by symmetry, we found that 2I = 2^{3/2} * ∫₀^{π/2} [1/(cos t + sin t)^2 ] dt

Then, after simplifying, we found that 2I = 2^{1/2} * [ -cot(t + π/4) ] from 0 to π/2

Which evaluated to 2^{1/2} * (1 +1) = 2^{3/2}

Therefore, 2I = 2^{3/2} ⇒ I = 2^{3/2}/2 = 2^{1/2} = √2

So the integral I is √2. Therefore, the original definite integral from 0 to 2 of x^{-1/2} [1 + sqrt(x(2 -x))]^{-3/2} dx equals √2.

Wait, let me confirm this. So after all substitutions and simplifications, the integral reduces to √2. Let me check with a numerical approximation to see if this makes sense.

Let's compute the numerical value of √2, which is approximately 1.41421356237. Let's check with a numerical integration method.

Alternatively, let's pick a value for x, say x=1. Then the integrand at x=1 is 1^{-1/2} [1 + sqrt(1*(2-1))]^{-3/2} = 1 * [1 +1]^{-3/2} = (2)^{-3/2} = 1/(2√2) ≈ 0.3535. The integral from 0 to 2 of this function. Since the function is symmetric around x=1, maybe the integral might indeed be √2. But let's approximate numerically.

Alternatively, let's use substitution x = 2 sin²θ. Wait, maybe another substitution. Let me try x = 2 sin²θ. Then dx = 4 sinθ cosθ dθ. When x=0, θ=0; x=2, θ=π/2. Then sqrt(x(2 -x)) = sqrt(2 sin²θ * 2 cos²θ) = sqrt(4 sin²θ cos²θ) = 2 sinθ cosθ. So the integrand becomes:

x^{-1/2} [1 + 2 sinθ cosθ]^{-3/2} dx

= (2 sin²θ)^{-1/2} [1 + 2 sinθ cosθ]^{-3/2} *4 sinθ cosθ dθ

= (sqrt(2) sinθ)^{-1} [1 + sin2θ]^{-3/2} *4 sinθ cosθ dθ

= (1/sqrt(2)) [1 + sin2θ]^{-3/2} *4 cosθ dθ

= (4/sqrt(2)) [1 + sin2θ]^{-3/2} cosθ dθ

= 2√2 [1 + sin2θ]^{-3/2} cosθ dθ

Hmm, but integrating this from θ=0 to π/2. Let's see. Let’s set u = 2θ, then du = 2 dθ. But not sure. Alternatively, let's set t = θ - π/4. But this might not help. Alternatively, note that 1 + sin2θ = (sinθ + cosθ)^2. So [1 + sin2θ]^{-3/2} = (sinθ + cosθ)^{-3}

So the integrand becomes 2√2 (sinθ + cosθ)^{-3} cosθ dθ

Hmm, integrating 2√2 ∫ cosθ / (sinθ + cosθ)^3 dθ from 0 to π/2. This seems similar to the previous integral we had. But we already found that the integral equals √2. So this substitution also leads to the same result. Therefore, the analytical result is √2.

Therefore, the exact answer is √2, and the numerical approximation is approximately 1.4142135624 when rounded to 10 decimal places.
</think>

{"answer": "\\sqrt{2}", "numerical_answer": "1.4142135624"}