To evaluate the definite integral

$$
\int_0^{\frac{1}{2}} \left\lfloor\frac{1}{x}\right\rfloor \left\lceil\frac{1}{x}\right\rceil \ln\left(1-\frac{1}{\left\lfloor\frac{1}{x}\right\rfloor^2}\right) \, dx,
$$

we begin by analyzing the structure of the integrand. The floor and ceiling functions suggest that the integrand is piecewise constant over intervals where $ \frac{1}{x} $ lies between consecutive integers. This motivates a change of variable.

---

### **Step 1: Substitution**

Let $ t = \frac{1}{x} \Rightarrow x = \frac{1}{t}, dx = -\frac{1}{t^2} dt $. When $ x \in (0, \frac{1}{2}] $, then $ t \in [2, \infty) $, and the integral becomes:

$$
\int_2^\infty \left\lfloor t \right\rfloor \left\lceil t \right\rceil \ln\left(1 - \frac{1}{\left\lfloor t \right\rfloor^2}\right) \cdot \frac{1}{t^2} \, dt.
$$

---

### **Step 2: Interval Analysis**

We observe that for each integer $ n \geq 2 $, the function $ \left\lfloor t \right\rfloor = n $ on the interval $ [n, n+1) $, and $ \left\lceil t \right\rceil = n+1 $ (except at the left endpoint $ t = n $, which has measure zero). Thus, the integrand is constant over each interval $ [n, n+1) $, and the integral becomes a sum:

$$
\sum_{n=2}^\infty \int_n^{n+1} n(n+1) \ln\left(1 - \frac{1}{n^2}\right) \cdot \frac{1}{t^2} \, dt.
$$

---

### **Step 3: Evaluate Each Integral**

$$
\int_n^{n+1} \frac{1}{t^2} dt = \left[-\frac{1}{t}\right]_n^{n+1} = \frac{1}{n} - \frac{1}{n+1}.
$$

So the $ n $-th term becomes:

$$
n(n+1) \ln\left(1 - \frac{1}{n^2}\right) \cdot \left(\frac{1}{n} - \frac{1}{n+1}\right)
= \ln\left(1 - \frac{1}{n^2}\right).
$$

Therefore, the entire integral reduces to:

$$
\sum_{n=2}^\infty \ln\left(1 - \frac{1}{n^2}\right).
$$

---

### **Step 4: Simplify the Infinite Sum**

We use the identity:

$$
\ln\left(1 - \frac{1}{n^2}\right) = \ln\left(\frac{n^2 - 1}{n^2}\right) = \ln(n^2 - 1) - \ln(n^2).
$$

This allows us to express the sum as a telescoping series:

$$
\sum_{n=2}^\infty \left[\ln(n^2 - 1) - \ln(n^2)\right] = \sum_{n=2}^\infty \left[\ln(n - 1) + \ln(n + 1) - 2\ln(n)\right].
$$

Grouping terms, we get:

$$
\sum_{n=2}^\infty \left[\ln(n - 1) - \ln(n)\right] + \sum_{n=2}^\infty \left[\ln(n + 1) - \ln(n)\right].
$$

Each of these sums telescopes:

- First sum: $ \ln(1) - \ln(2) + \ln(2) - \ln(3) + \cdots = -\ln(2) $,
- Second sum: $ \ln(3) - \ln(2) + \ln(4) - \ln(3) + \cdots = \lim_{N \to \infty} \ln(N+1) - \ln(2) \to \infty $.

However,