
To solve the definite integral \(\int_0^\pi \cos(x + \cos(x)) \, dx\), we proceed as follows:

### Step 1: Expand the integrand using trigonometric identities
Using the cosine addition formula \(\cos(A + B) = \cos A \cos B - \sin A \sin B\), we rewrite the integrand:
\[
\cos(x + \cos(x)) = \cos(x) \cos(\cos(x)) - \sin(x) \sin(\cos(x)).
\]
Thus, the integral splits into two parts:
\[
\int_0^\pi \cos(x + \cos(x)) \, dx = \int_0^\pi \cos(x) \cos(\cos(x)) \, dx - \int_0^\pi \sin(x) \sin(\cos(x)) \, dx.
\]

### Step 2: Evaluate the second integral (\(I_2\))
Let \(u = \cos(x)\), so \(du = -\sin(x) \, dx\). When \(x = 0\), \(u = 1\); when \(x = \pi\), \(u = -1\). Substituting, we get:
\[
\int_0^\pi \sin(x) \sin(\cos(x)) \, dx = \int_1^{-1} \sin(u) (-du) = \int_{-1}^1 \sin(u) \, du.
\]
The integral of \(\sin(u)\) over \([-1, 1]\) is zero because \(\sin(u)\) is an odd function and the interval is symmetric about the origin. Thus, \(I_2 = 0\).

### Step 3: Evaluate the first integral (\(I_1\))
Consider the substitution \(u = \pi - x\). Then \(du = -dx\), and when \(x = 0\), \(u = \pi\); when \(x = \pi\), \(u = 0\). Substituting, we get:
\[
I_1 = \int_0^\pi \cos(x) \cos(\cos(x)) \, dx = \int_\pi^0 \cos(\pi - u) \cos(\cos(\pi - u)) (-du).
\]
Simplifying \(\cos(\pi - u) = -\cos(u)\) and \(\cos(\cos(\pi - u)) = \cos(-\cos(u)) = \cos(\cos(u))\) (since cosine is even), we have:
\[
I_1 = \int_0^\pi -\cos(u) \cos(\cos(u)) \, du = -I_1.
\]
This implies \(2I_1 = 0\), so \(I_1 = 0\).

### Step 4: Combine results
The original integral is \(I_1 - I_2 = 0 - 0 = 0\).

### Numerical Approximation
The exact value is \(0\), so the numerical approximation is also \(0\) when rounded to 10 decimal places.

{"answer": "0", "numerical_answer": "0.0000000000"}