Let's solve the integral step by step:

\[
I = \int_0^{\pi/3}\frac{dx}{1+\tan^2(x)}
\]

Step 1: Simplify the integrand.

Recall that \( 1 + \tan^2(x) = \sec^2(x) \), so:

\[
I = \int_0^{\pi/3} \frac{dx}{\sec^2(x)} = \int_0^{\pi/3} \cos^2(x) dx
\]

However, actually,

\(
\frac{1}{1+\tan^2(x)} = \frac{1}{\sec^2(x)} = \cos^2(x)
\)

So the integral is:

\[
I = \int_0^{\pi/3} \cos^2(x) dx
\]

Step 2: Express \(\cos^2(x)\) with a double angle identity.
\[
\cos^2(x) = \frac{1+\cos(2x)}{2}
\]

So
\[
I = \int_0^{\pi/3} \frac{1+\cos(2x)}{2} dx
\]
\[
= \frac{1}{2} \int_0^{\pi/3} (1+\cos(2x)) dx
\]
\[
= \frac{1}{2} \left[ \int_0^{\pi/3} dx + \int_0^{\pi/3} \cos(2x) dx \right]
\]
\[
= \frac{1}{2} \left[ x \Big|_0^{\pi/3} + \left( \frac{1}{2}\sin(2x) \right) \Big|_0^{\pi/3} \right]
\]
\[
= \frac{1}{2} \left[ \frac{\pi}{3} - 0 + \frac{1}{2}(\sin(2\cdot\frac{\pi}{3})-\sin(0)) \right]
\]
\[
= \frac{1}{2} \left[ \frac{\pi}{3} + \frac{1}{2}\sin\left(\frac{2\pi}{3}\right) \right]
\]

Step 3: Compute \(\sin\left(\frac{2\pi}{3}\right)\).

\(
\sin\left(\frac{2\pi}{3}\right) = \sin\left(\pi - \frac{\pi}{3}\right) = \sin\left(\frac{\pi}{3}\right) = \frac{\sqrt{3}}{2}
\)

So the integral is:

\[
I = \frac{1}{2} \left[ \frac{\pi}{3} + \frac{1}{2} \cdot \frac{\sqrt{3}}{2} \right]
= \frac{1}{2} \left[ \frac{\pi}{3} + \frac{\sqrt{3}}{4} \right]
= \frac{\pi}{6} + \frac{\sqrt{3}}{8}
\]

Step 4: Numerical approximation.

Letâ€™s compute the approximation:

- \(\pi/6 \approx 0.5235987756\)
- \(\sqrt{3}/8 \approx 0.2165063509\)

Summing, \(0.5235987756 + 0.2165063509 = 0.7401051265\).

---

Final answer:
```json
{"answer": "\\frac{\\pi}{6} + \\frac{\\sqrt{3}}{8}", "numerical_answer": "0.7401051265"}
```