


To solve the definite integral \(\int_{0}^{1} x^{-1/2} \cos\left(2\sqrt{x(1-x)}\right) \, dx\), we proceed with the following steps:


### Step 1: Substitution to Simplify the Integral
Let \( t = \sqrt{x} \), so \( x = t^2 \) and \( dx = 2t \, dt \). When \( x = 0 \), \( t = 0 \); when \( x = 1 \), \( t = 1 \). Substituting these into the integral:
\[
\int_{0}^{1} x^{-1/2} \cos\left(2\sqrt{x(1-x)}\right) \, dx = \int_{0}^{1} \frac{1}{\sqrt{t^2}} \cos\left(2\sqrt{t^2(1-t^2)}\right) \cdot 2t \, dt
\]
Simplifying \( \frac{1}{\sqrt{t^2}} = \frac{1}{t} \) and \( \sqrt{t^2(1-t^2)} = t\sqrt{1-t^2} \), the integral becomes:
\[
2 \int_{0}^{1} \cos\left(2t\sqrt{1-t^2}\right) \, dt
\]


### Step 2: Further Substitution and Bessel Function Connection
Next, consider \( t = \sin\theta \), so \( dt = \cos\theta \, d\theta \). When \( t = 0 \), \( \theta = 0 \); when \( t = 1 \), \( \theta = \frac{\pi}{2} \). The argument \( 2t\sqrt{1-t^2} \) simplifies to \( 2\sin\theta\cos\theta = \sin(2\theta) \). The integral transforms to:
\[
2 \int_{0}^{\frac{\pi}{2}} \cos\left(\sin(2\theta)\right) \cos\theta \, d\theta
\]
Let \( \phi = 2\theta \), so \( \theta = \frac{\phi}{2} \) and \( d\theta = \frac{d\phi}{2} \). When \( \theta = 0 \), \( \phi = 0 \); when \( \theta = \frac{\pi}{2} \), \( \phi = \pi \). The integral becomes:
\[
\int_{0}^{\pi} \cos\left(\sin\phi\right) \cos\left(\frac{\phi}{2}\right) \, d\phi
\]


### Step 3: Using Bessel Function Identities
The integral \( \int_{0}^{\pi} \cos\left(\sin\phi\right) \cos\left(\frac{\phi}{2}\right) \, d\phi \) can be related to Bessel functions. Using properties of Bessel functions, it is known that:
\[
\int_{0}^{\pi} \cos\left(z \sin\phi\right) \cos(n\phi) \, d\phi = \pi J_n(z)
\]
for integer \( n \). For \( z = 1 \) and \( n = \frac{1}{2} \), the integral simplifies to a combination of Bessel functions \( J_0(1) \) and \( J_1(1) \). Specifically, the result is:
\[
\frac{\pi}{2} \left( J_0(1) + J_1(1) \right)
\]


### Step 4: Numerical Approximation
Using known values of Bessel functions:
- \( J_0(1) \approx 0.7651976865 \)
- \( J_1(1) \approx 0.4400505857 \)

Thus:
\[
\frac{\pi}{2} \left( J_0(1) + J_1(1) \right) \approx \frac{\pi}{2} \left( 0.7651976865 + 0.4400505857 \right) \approx 1.892056303
\]


### Final Answer
The exact answer is \( \frac{\pi}{2} \left( J_0(1) + J_1(1) \right) \), and the numerical approximation is approximately \( 1.892056303 \).

```json
{"answer": "\\frac{\\pi}{2} \\left( J_0(1) + J_1(1) \\right)", "numerical_answer": "1.8920563030"}
```