We start with the integral

  I = ∫₀¹ [ln(1 + x + x²) / x] dx.

Notice that the polynomial 1 + x + x² factors into the cubic factorization of x³ – 1. In fact, one can verify that

  x³ – 1 = (x – 1)(x² + x + 1),

so that

  1 + x + x² = (x³ – 1) / (x – 1).

On the interval x ∈ (0, 1) both x – 1 and x³ – 1 are negative and taking absolute values we have

  |1 + x + x²| = |(x³ – 1)/(x – 1)| = (1 – x³)/(1 – x).

Thus we may write
  ln(1 + x + x²) = ln[(1 – x³)/(1 – x)] = ln(1 – x³) – ln(1 – x).

Now, rewrite the original integral as

  I = ∫₀¹ [ln(1 – x³) – ln(1 – x)]/x dx.

Next, use the Taylor series expansion valid for |x| < 1:
  ln(1 – t) = –∑ₙ₌₁∞ tⁿ/n.

Apply this expansion with t = x and t = x³. Then
  ln(1 – x) = –∑ₙ₌₁∞ (xⁿ/n)
and
  ln(1 – x³) = –∑ₙ₌₁∞ (x³)ⁿ/n = –∑ₙ₌₁∞ (x^(3n)/n).

Thus, we have
  ln(1 – x³) – ln(1 – x) = ∑ₙ₌₁∞ [xⁿ – x^(3n)]/n.

Substitute this series expansion into I:

  I = ∫₀¹ [1/x] ∑ₙ₌₁∞ [xⁿ – x^(3n)]/n dx
    = ∑ₙ₌₁∞ (1/n) ∫₀¹ [xⁿ – x^(3n)]/x dx
    = ∑ₙ₌₁∞ (1/n) [∫₀¹ x^(n–1) dx – ∫₀¹ x^(3n–1) dx].

Since
  ∫₀¹ x^(k–1) dx = 1/k,
we get

  I = ∑ₙ₌₁∞ (1/n) [1/n – 1/(3n)] = ∑ₙ₌₁∞ (1/n)*[(3 – 1)/(3n)]
    = (2/3) ∑ₙ₌₁∞ 1/n².

The sum ∑ₙ₌₁∞ 1/n² is a well-known result equal to ζ(2) = π²/6. Thus

  I = (2/3)*(π²/6) = π²/9.

Numerically, π² is approximately 9.869604401089358, so

  I ≈ 9.869604401089358/9 ≈ 1.096622711232151.

Rounded to 10 decimal places, this is 1.0966227112.

{"answer": "\\frac{\\pi^2}{9}", "numerical_answer": "1.0966227112"}