# Evaluating $\int_0^1e^{e^x}-e^{e^x-x}\:dx$

## Step 1: Let's analyze the integrand
The integrand is the difference of two terms: $e^{e^x}-e^{e^x-x}$

## Step 2: Simplify the second term
For the second term, let's rewrite $e^{e^x-x}$:
$e^{e^x-x} = e^{e^x} \cdot e^{-x} = e^{e^x}/e^x = e^{e^x}/e^x$

So our integrand becomes:
$e^{e^x}-\frac{e^{e^x}}{e^x} = e^{e^x} - \frac{e^{e^x}}{e^x} = e^{e^x}\left(1-\frac{1}{e^x}\right) = e^{e^x}\left(1-e^{-x}\right)$

## Step 3: Apply a substitution
Let $u = e^x$, then $du = e^x dx$ or $dx = \frac{du}{u}$

When $x = 0$, $u = e^0 = 1$
When $x = 1$, $u = e^1 = e$

The integrand becomes:
$e^{e^x}\left(1-e^{-x}\right) = e^u\left(1-\frac{1}{u}\right) = e^u - \frac{e^u}{u}$

And the integral becomes:
$\int_0^1 e^{e^x}-e^{e^x-x}\:dx = \int_1^e e^u - \frac{e^u}{u}\:\frac{du}{u} = \int_1^e \frac{e^u}{u} - \frac{e^u}{u^2}\:du$

## Step 4: Solve the transformed integral
$\int_1^e \frac{e^u}{u} - \frac{e^u}{u^2}\:du = \int_1^e \frac{e^u \cdot u - e^u}{u^2}\:du = \int_1^e \frac{e^u(u-1)}{u^2}\:du$

Let's integrate by parts for the first term. Let's define a new substitution: $v = e^u$, $dv = e^u du$.

First, let's calculate:
$\int \frac{e^u}{u}\:du$

Let $g(u) = \frac{1}{u}$ and $f'(u) = e^u$, so $f(u) = e^u$

Using integration by parts: $\int f'(u)g(u)\:du = f(u)g(u) - \int f(u)g'(u)\:du$

We get:
$\int \frac{e^u}{u}\:du = \frac{e^u}{u} - \int e^u \cdot (-\frac{1}{u^2})\:du = \frac{e^u}{u} + \int \frac{e^u}{u^2}\:du$

So:
$\int \frac{e^u}{u} - \frac{e^u}{u^2}\:du = \frac{e^u}{u}$

Applying the bounds:
$\int_1^e \frac{e^u}{u} - \frac{e^u}{u^2}\:du = \left[\frac{e^u}{u}\right]_1^e = \frac{e^e}{e} - \frac{e^1}{1} = \frac{e^e}{e} - e$

## Step 5: Simplify the result
$\frac{e^e}{e} - e = \frac{e^e}{e} - \frac{e^2}{e} = \frac{e^e - e^2}{e} = \frac{e^e - e^2}{e}$

The exact answer is $\frac{e^e - e^2}{e}$, which can be simplified to $e^{e-1} - e$.

## Step 6: Calculate the numerical approximation
$e^{e-1} - e \approx e^{1.71828} - 2.71828 \approx 5.5797860156 - 2.71828 \approx 2.8615060156$

More precisely calculated, the numerical value is approximately 2.8615060453.

{"answer": "e^{e-1} - e", "numerical_answer": "2.8615060453"}