To solve the definite integral \(\int\limits_{0}^{\infty}\frac{x^{2}}{e^x-1}\left[2^{3}\sinh\left(0.5x\right)-\sinh\left(0.25x\right)\right]dx\), we will follow the steps outlined.

### Step 1: Simplify the integrand

First, let's simplify the expression inside the integral:
\[ 2^3 \sinh(0.5x) - \sinh(0.25x) = 8 \sinh(0.5x) - \sinh(0.25x). \]

Recall the definition of the hyperbolic sine function:
\[ \sinh(y) = \frac{e^y - e^{-y}}{2}. \]

Thus,
\[ 8 \sinh(0.5x) = 8 \cdot \frac{e^{0.5x} - e^{-0.5x}}{2} = 4(e^{0.5x} - e^{-0.5x}), \]
\[ \sinh(0.25x) = \frac{e^{0.25x} - e^{-0.25x}}{2}. \]

So the integrand becomes:
\[ \frac{x^2}{e^x - 1} \left[ 4(e^{0.5x} - e^{-0.5x}) - \frac{e^{0.25x} - e^{-0.25x}}{2} \right]. \]

### Step 2: Split the integral

We can split the integral into two parts:
\[ \int_0^\infty \frac{x^2}{e^x - 1} \left[ 4(e^{0.5x} - e^{-0.5x}) \right] dx - \int_0^\infty \frac{x^2}{e^x - 1} \left[ \frac{e^{0.25x} - e^{-0.25x}}{2} \right] dx. \]

### Step 3: Use known integral results

We use the known result for the integral involving the Bose-Einstein distribution:
\[ \int_0^\infty \frac{x^2 e^{-ax}}{e^x - 1} dx = 2 \Gamma(3) \zeta(3) a^{-3}, \]
where \(\Gamma(3) = 2!\) and \(\zeta(3)\) is the Riemann zeta function evaluated at 3.

For the first part:
\[ \int_0^\infty \frac{x^2 e^{-0.5x}}{e^x - 1} dx = 2 \Gamma(3) \zeta(3) (0.5)^{-3} = 2 \cdot 2 \cdot \zeta(3) \cdot 8 = 32 \zeta(3). \]

For the second part:
\[ \int_0^\infty \frac{x^2 e^{-0.25x}}{e^x - 1} dx = 2 \Gamma(3) \zeta(3) (0.25)^{-3} = 2 \cdot 2 \cdot \zeta(3) \cdot 64 = 256 \zeta(3). \]

### Step 4: Combine the results

Combining the results, we get:
\[ 4 \cdot 32 \zeta(3) - \frac{1}{2} \cdot 256 \zeta(3) = 128 \zeta(3) - 128 \zeta(3) = 0. \]

### Step 5: Numerical approximation

Since the exact result is 0, the numerical approximation is also 0.

### Final Answer

The final answer in the requested JSON format is:
```json
{"answer": "0", "numerical_answer": "0.0000000000"}
```