<think>
Okay, so I need to compute the definite integral of tanh(x) divided by e^x from 0 to infinity. Let me start by writing down the integral:

∫₀^∞ [tanh(x) / e^x] dx

First, I remember that tanh(x) is (e^x - e^(-x)) / (e^x + e^(-x)). Maybe substituting that in will help. Let me try that substitution.

So, tanh(x) = (e^x - e^(-x)) / (e^x + e^(-x)). Therefore, the integral becomes:

∫₀^∞ [(e^x - e^(-x)) / (e^x + e^(-x))] * e^(-x) dx

Let me simplify the expression inside the integral. Multiply the numerator and denominator by e^(-x) to make it easier. Wait, actually, let's first multiply the e^(-x) into the fraction. So, the integrand becomes:

[(e^x - e^(-x)) / (e^x + e^(-x))] * e^(-x) = [ (e^x - e^(-x)) * e^(-x) ] / (e^x + e^(-x))

Simplifying the numerator: e^x * e^(-x) = 1, and e^(-x) * e^(-x) = e^(-2x). So the numerator is 1 - e^(-2x). The denominator is e^x + e^(-x). So the integrand is (1 - e^(-2x)) / (e^x + e^(-x)).

Hmm, maybe that's a bit simpler. Let me write that:

Integral becomes ∫₀^∞ [1 - e^(-2x)] / (e^x + e^(-x)) dx

Alternatively, maybe factor e^(-x) in the denominator. Let's see:

Denominator: e^x + e^(-x) = e^(-x)(e^(2x) + 1). So, denominator is e^(-x)(e^(2x) + 1). Then the integrand is [1 - e^(-2x)] / [e^(-x)(e^(2x) + 1)] = [1 - e^(-2x)] * e^x / (e^(2x) + 1)

Wait, maybe that's a different approach. Let me check:

Wait, denominator e^x + e^(-x) = e^(-x)(e^(2x) + 1). So, [1 - e^(-2x)] / [e^(-x)(e^(2x) + 1)] = [1 - e^(-2x)] * e^x / (e^(2x) + 1)

So that's [e^x (1 - e^(-2x))] / (e^(2x) + 1) = [e^x - e^(-x)] / (e^(2x) + 1)

But that seems like going in circles. Maybe another substitution would help. Let me think.

Alternatively, perhaps use substitution t = e^(-x). Let's try that. Let t = e^(-x), so when x = 0, t = 1, and as x approaches infinity, t approaches 0. Then, dt = -e^(-x) dx, so dx = -dt / t.

Substituting into the integral:

Original integral becomes ∫ from t=1 to t=0 of [tanh(-ln t)] * t * (-dt/t)

Wait, tanh(x) where x = -ln t. Let's compute tanh(-ln t). Since tanh is odd, tanh(-ln t) = -tanh(ln t). So:

Integral becomes ∫ from 1 to 0 of [-tanh(ln t)] * t * (-dt/t) = ∫ from 1 to 0 of tanh(ln t) * (t / t) dt? Wait, let me check again.

Wait, x = -ln t, so tanh(x) = tanh(-ln t) = -tanh(ln t). Then, the integrand is [ -tanh(ln t) ] * t, because e^(-x) = t. Then, dx = -dt/t.

So the integral becomes:

∫ (from t=1 to t=0) [ -tanh(ln t) ] * t * (-dt/t )

The two negatives make a positive, and the t cancels with the 1/t from dx. So:

∫ from 1=1 to t2=0 of tanh(ln t) dt. But integrating from 1 to 0 is the same as integrating from 0 to 1 with a negative sign. So:

= ∫ from 0 to 1 of tanh(ln t) dt

Hmm, not sure if that's better. Let's compute tanh(ln t). Let me recall that tanh(z) = (e^z - e^(-z)) / (e^z + e^(-z)). So, if z = ln t, then:

tanh(ln t) = (t - 1/t) / (t + 1/t) = (t^2 - 1) / (t^2 + 1)

So, substituting back, the integral becomes:

∫₀¹ [ (t² - 1) / (t² + 1) ] dt

That seems more manageable. Let's compute this integral:

∫₀¹ (t² - 1)/(t² + 1) dt

We can split the numerator:

= ∫₀¹ [ (t² + 1 - 2) / (t² + 1) ] dt = ∫₀¹ [1 - 2/(t² + 1)] dt

So, integrating term by term:

= ∫₀¹ 1 dt - 2 ∫₀¹ 1/(t² + 1) dt

Compute each integral:

First integral: ∫₀¹ 1 dt = 1 - 0 = 1

Second integral: ∫₀¹ 1/(t² + 1) dt = arctan(t) from 0 to 1 = arctan(1) - arctan(0) = π/4 - 0 = π/4

So, putting it all together:

1 - 2*(π/4) = 1 - π/2

Wait, but that's the integral from 0 to 1 of [ (t² -1)/(t² +1) ] dt. But remember, this was after substitution, which was equal to the original integral. So, the original integral from 0 to infinity of tanh(x)/e^x dx equals 1 - π/2?

Wait, but wait, let me check the substitution steps again to make sure.

Original substitution: t = e^(-x), so x = -ln t, dx = -dt/t. Then, the integral becomes:

∫₀^∞ [tanh(x)/e^x] dx = ∫₀¹ tanh(-ln t) * t * ( -dt/t )

Wait, let's redo this substitution step by step.

Original integral: ∫₀^∞ [tanh(x) e^{-x}] dx

Let t = e^{-x}, so x = -ln t, dx = -dt/t. When x=0, t=1; x→infty, t→0.

So substituting:

Integral becomes ∫_{t=1}^{t=0} tanh(-ln t) * t * (-dt/t )

Simplify the expression:

tanh(-ln t) = -tanh(ln t) because tanh is odd.

So, the integrand becomes (-tanh(ln t)) * t * (-dt/t) = tanh(ln t) * dt

The limits are from 1 to 0, so we can reverse them and remove the negative sign:

= ∫₀¹ tanh(ln t) dt

Then, as before, tanh(ln t) = (t - 1/t)/(t + 1/t) = (t² -1)/(t² +1)

So, integral becomes ∫₀¹ (t² -1)/(t² +1) dt = 1 - π/2

Wait, but 1 - π/2 is negative because π ≈ 3.1416, so π/2 ≈ 1.5708, so 1 - 1.5708 ≈ -0.5708. But the original integrand is tanh(x)/e^x. Since tanh(x) is positive for x >0, and e^x is positive, the integrand is positive, so the integral should be positive. But here we get a negative value. That can't be right. So there must be a mistake in the substitution.

Wait, so where did I go wrong?

Let me check the substitution again. The original integral is ∫₀^∞ [tanh(x)/e^x] dx. Let me check the substitution steps again.

Let t = e^{-x}, so x = -ln t, dx = -dt/t. Then, when x=0, t=1; x=infty, t=0.

So, substituting into the integral:

∫₀^∞ [tanh(x) e^{-x}] dx = ∫_{1}^{0} tanh(-ln t) * t * (-dt/t )

Simplify the terms:

tanh(-ln t) = -tanh(ln t)

Then, the integrand becomes (-tanh(ln t)) * t * (-dt/t) = tanh(ln t) * dt

But the limits are from 1 to 0, so reversing them gives:

= ∫₀¹ tanh(ln t) dt

But tanh(ln t) = (t - 1/t)/(t + 1/t) = (t² -1)/(t² +1)

So, the integral becomes ∫₀¹ (t² -1)/(t² +1) dt

But (t² -1)/(t² +1) = 1 - 2/(t² +1), so integrating from 0 to1:

= [ t - 2 arctan(t) ] from 0 to1

At t=1: 1 - 2*(π/4) = 1 - π/2

At t=0: 0 - 2*0 = 0

So the integral is (1 - π/2) - 0 = 1 - π/2 ≈ 1 - 1.5708 ≈ -0.5708

But the original integral is of a positive function, so the result should be positive. Therefore, there's a mistake here. Where?

Wait, perhaps the substitution step is incorrect. Let me check the substitution again.

Original integral: ∫₀^∞ [tanh(x)/e^x] dx

Substitute t = e^{-x}, so x = -ln t, dx = -dt/t. Then, e^{-x} = t. So, the integrand becomes tanh(x) * t. But x is -ln t, so tanh(-ln t) = -tanh(ln t). Therefore, the integrand is -tanh(ln t) * t. Then, dx = -dt/t. So putting it all together:

∫₀^∞ [tanh(x)/e^x] dx = ∫_{1}^{0} [ -tanh(ln t) * t ] * (-dt/t )

Let's compute the terms inside the integral:

[ -tanh(ln t) * t ] * (-dt/t ) = [ -tanh(ln t) * t ] * (-1/t) dt = tanh(ln t) dt

So the integral becomes ∫_{1}^{0} tanh(ln t) dt = -∫_{0}^{1} tanh(ln t) dt

Wait, but earlier I thought it was ∫₀¹, but here it's ∫₁⁰ which is -∫₀¹. So the integral is -∫₀¹ tanh(ln t) dt. But earlier, I had ∫₀¹ tanh(ln t) dt = 1 - π/2, so the original integral would be - (1 - π/2) = π/2 -1 ≈ 0.5708, which is positive. That makes sense.

Ah! There was a sign error in the substitution. So the correct result is π/2 -1. That's positive. So the mistake was in the substitution limits. When I did the substitution, the integral became ∫₁⁰ ... which is -∫₀¹ ... So the integral is - (1 - π/2) = π/2 -1.

So the correct value is π/2 -1. Let me confirm this.

Yes, because when you substitute t = e^{-x}, the integral becomes from t=1 to t=0, which is the negative of from 0 to1. So the integral is - [1 - π/2] = π/2 -1. So the original integral is π/2 -1.

Therefore, the exact answer is π/2 -1.

Now, let's compute the numerical approximation. π is approximately 3.1415926536, so π/2 ≈ 1.5707963268. Then, π/2 -1 ≈ 0.5707963268. Rounded to 10 decimal places, that's approximately 0.5707963268.

Wait, let me check with a calculator. 3.141592653589793 / 2 = 1.5707963267948966. Subtract 1 gives 0.5707963267948966. So, approximately 0.5707963268 when rounded to 10 decimal places.

Alternatively, the exact value is π/2 -1, and numerically that's approximately 0.5707963267948966...

So, the final answer is π/2 -1, and the numerical approximation is approximately 0.5707963268.

Let me verify this result another way to be sure. Maybe expand tanh(x) as a series and integrate term by term.

Recall that tanh(x) can be expressed as 1 - 2/(e^{2x} +1). So:

tanh(x) = 1 - 2/(e^{2x} +1)

Therefore, the integrand becomes [1 - 2/(e^{2x} +1)] * e^{-x} = e^{-x} - 2 e^{-x}/(e^{2x} +1)

So, the integral from 0 to ∞ is:

∫₀^∞ e^{-x} dx - 2 ∫₀^∞ e^{-x}/(e^{2x} +1) dx

First integral: ∫₀^∞ e^{-x} dx = 1

Second integral: 2 ∫₀^∞ e^{-x}/(e^{2x} +1) dx. Let me compute this.

Let me make substitution t = e^{-x}, so when x=0, t=1; x→∞, t→0. Then, dt = -e^{-x} dx, so dx = -dt/t.

So, the second integral becomes:

2 ∫_{1}^{0} t / ( (1/t^2) +1 ) * (-dt/t )

Wait, e^{2x} = (e^{-x})^{-2} = t^{-2}

So, denominator e^{2x} +1 = t^{-2} +1 = (1 + t^2)/t^2

Therefore, 1/(e^{2x} +1) = t^2/(1 + t^2)

So, the integrand e^{-x}/(e^{2x} +1) = t * t^2/(1 + t^2) = t^3/(1 + t^2)

But let's go through the substitution step carefully.

Original integral: ∫₀^∞ e^{-x}/(e^{2x} +1) dx

Substitute t = e^{-x}, so x = -ln t, dx = -dt/t. Then, e^{-x} = t, e^{2x} = e^{-2 ln t} = t^{-2}

So, the integral becomes:

∫_{t=1}^{t=0} [ t / (t^{-2} +1) ] * (-dt/t )

Simplify:

t / (t^{-2} +1) = t / ( (1 + t^2)/t^2 ) ) = t * t^2 / (1 + t^2) ) = t^3 / (1 + t^2)

Then, the integral becomes:

∫₁⁰ [ t^3 / (1 + t^2) ] * (-dt/t ) = ∫₀¹ [ t^3 / (1 + t^2) ] * (dt/t )

Simplify the integrand:

t^3 / t = t^2, so:

= ∫₀¹ t^2 / (1 + t^2) dt

Which is ∫₀¹ [1 - 1/(1 + t^2)] dt

So, integrating from 0 to1:

= [ t - arctan(t) ] from 0 to1 = (1 - π/4) - (0 -0) = 1 - π/4

Therefore, the second integral is 2*(1 - π/4)

So, the original integral is 1 - 2*(1 - π/4) = 1 - 2 + π/2 = π/2 -1, which matches the previous result. So that's correct.

Therefore, the exact value is π/2 -1, and the numerical value is approximately 0.5707963268.

So, the answer is π/2 -1, and the numerical approximation is approximately 0.5707963268.
</think>

{"answer": "\\frac{\\pi}{2} - 1", "numerical_answer": "0.5707963268"}