# Evaluating the definite integral $\int_0^{\frac{1}{2}}\left\lfloor\frac{1}{x}\right\rfloor\left\lceil\frac{1}{x}\right\rceil\ln\left(1-\frac{1}{\left\lfloor\frac{1}{x}\right\rfloor^2}\right)\mathrm{d}x$

## Step 1: Analyzing the domain and identifying intervals

For $x \in (0, \frac{1}{2}]$, we have $\frac{1}{x} \geq 2$. Let's break down the interval based on the values of $\left\lfloor\frac{1}{x}\right\rfloor$:

- When $x \in (\frac{1}{3}, \frac{1}{2}]$, we have $2 \leq \frac{1}{x} < 3$, so $\left\lfloor\frac{1}{x}\right\rfloor = 2$ and $\left\lceil\frac{1}{x}\right\rceil = 3$
- When $x \in (\frac{1}{4}, \frac{1}{3}]$, we have $3 \leq \frac{1}{x} < 4$, so $\left\lfloor\frac{1}{x}\right\rfloor = 3$ and $\left\lceil\frac{1}{x}\right\rceil = 4$
- And so on...

Let's rewrite the integral as a sum of integrals over these intervals:

$$\int_0^{\frac{1}{2}}\left\lfloor\frac{1}{x}\right\rfloor\left\lceil\frac{1}{x}\right\rceil\ln\left(1-\frac{1}{\left\lfloor\frac{1}{x}\right\rfloor^2}\right)\mathrm{d}x = \sum_{n=2}^{\infty}\int_{\frac{1}{n+1}}^{\frac{1}{n}}n(n+1)\ln\left(1-\frac{1}{n^2}\right)\mathrm{d}x$$

## Step 2: Simplifying each integral in the sum

For each $n \geq 2$, we have:

$$\int_{\frac{1}{n+1}}^{\frac{1}{n}}n(n+1)\ln\left(1-\frac{1}{n^2}\right)\mathrm{d}x = n(n+1)\ln\left(1-\frac{1}{n^2}\right)\int_{\frac{1}{n+1}}^{\frac{1}{n}}\mathrm{d}x$$

Since $\int_{\frac{1}{n+1}}^{\frac{1}{n}}\mathrm{d}x = \frac{1}{n} - \frac{1}{n+1} = \frac{1}{n(n+1)}$, we get:

$$\int_{\frac{1}{n+1}}^{\frac{1}{n}}n(n+1)\ln\left(1-\frac{1}{n^2}\right)\mathrm{d}x = \ln\left(1-\frac{1}{n^2}\right)$$

## Step 3: Computing the infinite sum

Our integral becomes:

$$\int_0^{\frac{1}{2}}\left\lfloor\frac{1}{x}\right\rfloor\left\lceil\frac{1}{x}\right\rceil\ln\left(1-\frac{1}{\left\lfloor\frac{1}{x}\right\rfloor^2}\right)\mathrm{d}x = \sum_{n=2}^{\infty}\ln\left(1-\frac{1}{n^2}\right)$$

Using the property of logarithms, $\ln\left(1-\frac{1}{n^2}\right) = \ln\left(\frac{n^2-1}{n^2}\right) = \ln\left(\frac{(n-1)(n+1)}{n^2}\right)$:

$$\sum_{n=2}^{\infty}\ln\left(1-\frac{1}{n^2}\right) = \sum_{n=2}^{\infty}\ln\left(\frac{(n-1)(n+1)}{n^2}\right) = \sum_{n=2}^{\infty}\ln\left(\frac{n-1}{n}\cdot\frac{n+1}{n}\right)$$

This simplifies to:

$$\sum_{n=2}^{\infty}\ln\left(\frac{n-1}{n}\right) + \sum_{n=2}^{\infty}\ln\left(\frac{n+1}{n}\right)$$

## Step 4: Manipulating the telescoping series

The first sum is:
$$\sum_{n=2}^{\infty}\ln\left(\frac{n-1}{n}\right) = \ln\left(\frac{1}{2}\right) + \ln\left(\frac{2}{3}\right) + \ln\left(\frac{3}{4}\right) + \ldots$$

The second sum is:
$$\sum_{n=2}^{\infty}\ln\left(\frac{n+1}{n}\right) = \ln\left(\frac{3}{2}\right) + \ln\left(\frac{4}{3}\right) + \ln\left(\frac{5}{4}\right) + \ldots$$

Looking at the combined series, most terms cancel out in a telescoping fashion, leaving:
$$\ln\left(\frac{1}{2}\right) + \ln\left(\frac{3}{2}\right) = \ln\left(\frac{3}{4}\right)$$

## Step 5: Final result

The definite integral evaluates to:
$$\int_0^{\frac{1}{2}}\left\lfloor\frac{1}{x}\right\rfloor\left\lceil\frac{1}{x}\right\rceil\ln\left(1-\frac{1}{\left\lfloor\frac{1}{x}\right\rfloor^2}\right)\mathrm{d}x = \ln\left(\frac{3}{4}\right)$$

The numerical approximation of $\ln\left(\frac{3}{4}\right)$ rounded to 10 decimal places is:
$\ln\left(\frac{3}{4}\right) = -0.2876820725$

{"answer": "\\ln\\left(\\frac{3}{4}\\right)", "numerical_answer": "-0.2876820725"}