

To calculate the definite integral \(\int_0^{2\pi}\left|1+2\sin x\right|dx\), we follow these steps:

### Step 1: Identify where \(1 + 2\sin x\) is positive or negative
The expression inside the absolute value, \(1 + 2\sin x\), changes sign where \(1 + 2\sin x = 0\). Solving for \(x\):
\[
1 + 2\sin x = 0 \implies \sin x = -\frac{1}{2}
\]
In the interval \([0, 2\pi)\), the solutions are \(x = \frac{7\pi}{6}\) and \(x = \frac{11\pi}{6}\). These points divide \([0, 2\pi)\) into three subintervals:
- \(0 \leq x < \frac{7\pi}{6}\): \(1 + 2\sin x > 0\)
- \(\frac{7\pi}{6} \leq x < \frac{11\pi}{6}\): \(1 + 2\sin x < 0\)
- \(\frac{11\pi}{6} \leq x \leq 2\pi\): \(1 + 2\sin x > 0\)

### Step 2: Split the integral based on sign changes
The integral becomes:
\[
\int_0^{2\pi}\left|1+2\sin x\right|dx = \int_0^{\frac{7\pi}{6}} (1 + 2\sin x)dx + \int_{\frac{7\pi}{6}}^{\frac{11\pi}{6}} -(1 + 2\sin x)dx + \int_{\frac{11\pi}{6}}^{2\pi} (1 + 2\sin x)dx
\]

### Step 3: Evaluate each sub-integral
#### First integral (\(0\) to \(\frac{7\pi}{6}\)):
\[
\int_0^{\frac{7\pi}{6}} (1 + 2\sin x)dx = \left[x - 2\cos x\right]_0^{\frac{7\pi}{6}}
\]
At \(x = \frac{7\pi}{6}\): \(x - 2\cos x = \frac{7\pi}{6} - 2\left(-\frac{\sqrt{3}}{2}\right) = \frac{7\pi}{6} + \sqrt{3}\)  
At \(x = 0\): \(x - 2\cos x = 0 - 2(1) = -2\)  
Thus: \(\frac{7\pi}{6} + \sqrt{3} - (-2) = \frac{7\pi}{6} + \sqrt{3} + 2\)

#### Second integral (\(\frac{7\pi}{6}\) to \(\frac{11\pi}{6}\)):
\[
\int_{\frac{7\pi}{6}}^{\frac{11\pi}{6}} -(1 + 2\sin x)dx = \int_{\frac{7\pi}{6}}^{\frac{11\pi}{6}} (-1 - 2\sin x)dx = \left[-x + 2\cos x\right]_{\frac{7\pi}{6}}^{\frac{11\pi}{6}}
\]
At \(x = \frac{11\pi}{6}\): \(-x + 2\cos x = -\frac{11\pi}{6} + 2\left(\frac{\sqrt{3}}{2}\right) = -\frac{11\pi}{6} + \sqrt{3}\)  
At \(x = \frac{7\pi}{6}\): \(-x + 2\cos x = -\frac{7\pi}{6} + 2\left(-\frac{\sqrt{3}}{2}\right) = -\frac{7\pi}{6} - \sqrt{3}\)  
Thus: \(\left(-\frac{11\pi}{6} + \sqrt{3}\right) - \left(-\frac{7\pi}{6} - \sqrt{3}\right) = -\frac{2\pi}{3} + 2\sqrt{3}\)

#### Third integral (\(\frac{11\pi}{6}\) to \(2\pi\)):
\[
\int_{\frac{11\pi}{6}}^{2\pi} (1 + 2\sin x)dx = \left[x - 2\cos x\right]_{\frac{11\pi}{6}}^{2\pi}
\]
At \(x = 2\pi\): \(x - 2\cos x = 2\pi - 2(1) = 2\pi - 2\)  
At \(x = \frac{11\pi}{6}\): \(x - 2\cos x = \frac{11\pi}{6} - 2\left(\frac{\sqrt{3}}{2}\right) = \frac{11\pi}{6} - \sqrt{3}\)  
Thus: \((2\pi - 2) - \left(\frac{11\pi}{6} - \sqrt{3}\right) = \frac{\pi}{6} - 2 + \sqrt{3}\)

### Step 4: Sum the results
Adding the three sub-integrals:
\[
\left(\frac{7\pi}{6} + \sqrt{3} + 2\right) + \left(-\frac{2\pi}{3} + 2\sqrt{3}\right) + \left(\frac{\pi}{6} - 2 + \sqrt{3}\right)
\]
Simplifying:
- \(\pi\) terms: \(\frac{7\pi}{6} - \frac{2\pi}{3} + \frac{\pi}{6} = \frac{2\pi}{3}\)
- \(\sqrt{3}\) terms: \(\sqrt{3} + 2\sqrt{3} + \sqrt{3} = 4\sqrt{3}\)
- Constants: \(2 - 2 = 0\)

Thus, the exact value is \(\frac{2\pi}{3} + 4\sqrt{3}\).

### Step 5: Numerical approximation
Using \(\pi \approx 3.141592653589793\) and \(\sqrt{3} \approx 1.7320508075688772\):
\[
\frac{2\pi}{3} + 4\sqrt{3} \approx 2.0943951024 + 6.9282032303 = 9.0225983327
\]

{"answer": "\\frac{2\\pi}{3} + 4\\sqrt{3}", "numerical_answer": "9.0225983327"}