Let's proceed step by step:

Let
\[
I = \int_{0}^{\infty} \frac{e^{-ax}}{\sqrt{x}} \left[ \sin x\, \mathrm{Ci}(2x) - \cos x\, \mathrm{Si}(2x) \right] dx
\]
where \( a = 1.0 \).

**Step 1: Analytical Solution**

This is a special integral involving exponential, trigonometric, sine and cosine integrals, and a fractional power.

Recall:
- \(\mathrm{Si}(z) = \int_0^z \frac{\sin t}{t} dt\)
- \(\mathrm{Ci}(z) = -\int_z^\infty \frac{\cos t}{t} dt\)

A key approach is to relate this integral to Laplace transforms or known integrals.

Let’s reference Gradshteyn & Ryzhik 3.944 or 3.954, as well as other tables.

In Gradshteyn & Ryzhik 3.944.2:
\[
\int_{0}^{\infty} x^{\mu-1} e^{-\beta x} \Big[ \sin(\alpha x) \, \mathrm{Ci}(\gamma x) - \cos(\alpha x) \, \mathrm{Si}(\gamma x) \Big] dx = \frac{\Gamma(\mu) \sin(\pi \mu)}{2} \int_{0}^{\gamma} \frac{dt}{(t + \beta + i\alpha)^{\mu}}
\]
for certain parameters.

In our case:

- \(\mu = 1/2\)
- \(\beta = a = 1.0\)
- \(\alpha = 1\)
- \(\gamma = 2\)

So,
\[
I = \int_{0}^{\infty} x^{-1/2} e^{-a x} \big[ \sin x\, \mathrm{Ci}(2x) - \cos x\, \mathrm{Si}(2x) \big] dx
\]

According to the table, we have:

\[
\int_{0}^{\infty} x^{\mu-1} e^{-\beta x} \Big[ \sin(\alpha x) \, \mathrm{Ci}(\gamma x) - \cos(\alpha x) \, \mathrm{Si}(\gamma x) \Big] dx = \Gamma(\mu)\, \Im \int_{0}^{\gamma} \frac{dt}{(t + \beta + i\alpha)^{\mu}}
\]

Here, \(\Im\) denotes the imaginary part.

Plug in the values:
- \(\Gamma(1/2) = \sqrt{\pi}\)
- \(\mu = 1/2\)

So,
\[
I = \sqrt{\pi}\, \Im \int_{0}^{2} \frac{dt}{(t + 1 + i)^{1/2}}
\]

Let’s write \(z = t + 1 + i\), so:
\[
I = \sqrt{\pi} \cdot \Im \int_{t=0}^{2} (t + 1 + i)^{-1/2} dt
\]

Alternatively, integrate via substitution.

Write \(z = t + 1 + i\):

Let’s parametrize \(t\) from 0 to 2:

- When \(t=0\): \(z_0 = 1 + i\)
- When \(t=2\): \(z_1 = 3 + i\)

Let’s recall:

\[
\int z^{\alpha} dz = \frac{1}{\alpha+1} z^{\alpha+1}
\]

So
\[
\int (t + 1 + i)^{-1/2} dt = \int (z)^{-1/2} dt = \int (z)^{-1/2} dz \cdot \frac{dt}{dz}
\]
But \(dt = dz\), so:

So,
\[
\int_{t=0}^2 (t + 1 + i)^{-1/2} dt = \int_{z=1+i}^{3+i} z^{-1/2} dz
= 2 \left[ z^{1/2} \right]_{z=1+i}^{3+i}
\]

So,
\[
\int_{0}^{2} (t + 1 + i)^{-1/2} dt = 2 \left[ (3 + i)^{1/2} - (1 + i)^{1/2} \right]
\]

Therefore,
\[
I = \sqrt{\pi} \cdot \Im \left\{ 2 \left[ (3+i)^{1/2} - (1+i)^{1/2} \right] \right\}
\]
\[
= 2\sqrt{\pi} \cdot \Im \left[ (3+i)^{1/2} - (1+i)^{1/2} \right]
\]

Now, compute the square roots and take the imaginary part.

Let’s compute \( (1+i)^{1/2} \):

\(1 + i = \sqrt{2}\, e^{i\pi/4}\)

So
\[
(1+i)^{1/2} = (\sqrt{2})^{1/2} e^{i\pi/8} = 2^{1/4} \left[ \cos\frac{\pi}{8} + i \sin\frac{\pi}{8} \right]
\]
Similarly, \(3 + i\):

Compute modulus:
\[
|3+i| = \sqrt{9+1} = \sqrt{10}
\]

Arg:
\[
\theta = \arctan(1/3)
\]

Therefore,
\[
(3+i)^{1/2} = (\sqrt{10})^{1/2} e^{i \arctan(1/3)/2}
= 10^{1/4} \left[ \cos \frac{1}{2} \arctan(1/3) + i \sin \frac{1}{2} \arctan(1/3) \right]
\]

So,
\[
I = 2\sqrt{\pi} \left[ \Im (3+i)^{1/2} - \Im (1+i)^{1/2} \right]
\]

**Step 2: Explicit Result**

Plugging into above:

- \((1+i):\) argument = \(\pi/4\), modulus = \(\sqrt{2}\)
\[
(1+i)^{1/2} = 2^{1/4} \left( \cos \frac{\pi}{8} + i \sin \frac{\pi}{8} \right)
\]
So the imaginary part is \(2^{1/4} \sin \frac{\pi}{8}\)

- \((3+i):\) modulus \(= \sqrt{10}\), argument \(= \arctan(1/3)\)

Let’s denote \(\varphi = \arctan(1/3)\) so \(\tan \varphi = 1/3\)

So,
\[
(3+i)^{1/2} = 10^{1/4} \left( \cos \frac{\varphi}{2} + i \sin \frac{\varphi}{2} \right)
\]
Imaginary part is \(10^{1/4} \sin \frac{\varphi}{2}\)

Putting it together,
\[
I = 2 \sqrt{\pi} \left[ 10^{1/4} \sin \frac{\arctan(1/3)}{2} - 2^{1/4} \sin \frac{\pi}{8} \right]
\]

**Step 3: Numerical evaluation**

Let’s compute everything step by step (rounded to 10 decimals):

- \(2^{1/4} = \sqrt{\sqrt{2}} \approx 1.1892071150\)
- \(\sin(\pi/8) \approx \sin(22.5^\circ) \approx 0.3826834324\)

Next,

- \(\arctan(1/3) \approx 0.3217505544\) radians
- So half that: \(0.1608752772\) radians

- \(10^{1/4} = (10^{1/2})^{1/2} = (\sqrt{10})^{1/2} \approx (3.1622776602)^{1/2} \approx 1.7782794100\)
- \(\sin(0.1608752772) \approx 0.1601391853\)

So,
- \(10^{1/4} \sin(\arctan(1/3)/2) \approx 1.7782794100 \times 0.1601391853 \approx 0.2848097278\)

- \(2^{1/4} \sin(\pi/8) \approx 1.1892071150 \times 0.3826834324 \approx 0.4550898606\)

Now subtract:

\(0.2848097278 - 0.4550898606 = -0.1702801328\)

Multiply by \(2\sqrt{\pi}\):

\(\sqrt{\pi} \approx 1.7724538509\)

\(2 \sqrt{\pi} \approx 3.5449077018\)

So final result:

\(3.5449077018 \times (-0.1702801328) \approx -0.6038786622\)

**Step 4: JSON Output**

```json
{"answer": "2 \\sqrt{\\pi}\\left[10^{1/4}\\sin\\left(\\frac{1}{2}\\arctan\\frac{1}{3}\\right)-2^{1/4}\\sin\\left(\\frac{\\pi}{8}\\right)\\right]", "numerical_answer": "-0.6038786622"}
```