Given the integral:
\[
I = \int_{0}^{2} x^{-1/2} (2-x)^{-1/2} [1-0.5x(2-x)] dx
\]

Let's proceed step by step.

---

**Step 1: Simplification**

Let us expand the bracket:
\[
1 - 0.5x(2-x) = 1 - x + 0.5x^2
\]
So the integral can be rewritten as:
\[
I = \int_0^2 x^{-1/2}(2-x)^{-1/2}(1 - x + 0.5x^2) dx
\]
Distribute:
\[
I = \int_0^2 x^{-1/2}(2-x)^{-1/2}dx 
  - \int_0^2 x^{1/2}(2-x)^{-1/2}dx 
  + 0.5\int_0^2 x^{3/2}(2-x)^{-1/2} dx
\]

Let us denote:
\[
I_1 = \int_0^2 x^{-1/2}(2-x)^{-1/2}dx
\]
\[
I_2 = \int_0^2 x^{1/2}(2-x)^{-1/2}dx
\]
\[
I_3 = \int_0^2 x^{3/2}(2-x)^{-1/2}dx
\]
So:
\[
I = I_1 - I_2 + 0.5I_3
\]

---

## Compute \(I_1\), \(I_2\), and \(I_3\):

### \(I_1\):

\[
I_1 = \int_0^2 x^{-1/2}(2-x)^{-1/2}dx
\]

Let \(x = 2t\), \(dx = 2dt\), as \(x\) goes from \(0\) to \(2\), \(t\) goes from \(0\) to \(1\).

Substitute:
\[
x^{-1/2} = (2t)^{-1/2} = 2^{-1/2} t^{-1/2}
\]
\[
2-x = 2-2t = 2(1-t) \implies (2-x)^{-1/2} = 2^{-1/2}(1-t)^{-1/2}
\]
So,
\[
I_1 = \int_{x=0}^{x=2} x^{-1/2} (2-x)^{-1/2} dx
= \int_{t=0}^{t=1} 2^{-1/2} t^{-1/2} \cdot 2^{-1/2} (1-t)^{-1/2} \cdot 2 dt
\]
\[
= 2^{-1} \cdot t^{-1/2}(1-t)^{-1/2} \cdot 2 dt
= \int_{0}^{1} t^{-1/2}(1-t)^{-1/2}dt
\]
This is the Beta function:
\[
\int_0^1 t^{a-1}(1-t)^{b-1}dt = \mathrm{B}(a, b) = \frac{\Gamma(a)\Gamma(b)}{\Gamma(a + b)}
\]
For \(a = b = 1/2\):
\[
I_1 = \mathrm{B}(1/2, 1/2) = \frac{\Gamma(1/2)\Gamma(1/2)}{\Gamma(1)}
= \frac{\pi}{1} = \pi
\]

---

### \(I_2\):

\[
I_2 = \int_0^2 x^{1/2}(2-x)^{-1/2} dx
\]
Again, use the substitution \(x = 2t\), \(dx = 2dt\), \(t\) from 0 to 1.
\[
x^{1/2} = (2t)^{1/2} = 2^{1/2} t^{1/2}
\]
\[
(2-x)^{-1/2} = [2(1-t)]^{-1/2} = 2^{-1/2} (1-t)^{-1/2}
\]
Plug these in:
\[
I_2 = \int_{t=0}^{t=1} 2^{1/2} t^{1/2} \cdot 2^{-1/2} (1-t)^{-1/2} \cdot 2 dt
= \int_0^1 t^{1/2}(1-t)^{-1/2} \cdot 2 dt
\]
\[
= 2 \int_0^1 t^{1/2}(1-t)^{-1/2}dt
\]
Beta function:
\[
\int_0^1 t^{a-1}(1-t)^{b-1}dt = \mathrm{B}(a, b)
\]
Here, \(a = 3/2\), \(b = 1/2\):
\[
I_2 = 2 \cdot \mathrm{B}(3/2, 1/2) = 2\frac{\Gamma(3/2)\Gamma(1/2)}{\Gamma(2)}
\]
Recall:
\[
\Gamma(1/2) = \sqrt{\pi}
\]
\[
\Gamma(3/2) = (1/2)\Gamma(1/2) = (1/2)\sqrt{\pi}
\]
\[
\Gamma(2) = 1!
\]
So,
\[
I_2 = 2 \cdot \frac{(1/2)\sqrt{\pi}\cdot \sqrt{\pi}}{1}
= 2 \cdot \frac{1}{2} \pi
= \pi
\]

---

### \(I_3\):

\[
I_3 = \int_0^{2} x^{3/2} (2-x)^{-1/2} dx
\]
Same substitution: \(x=2t\), \(dx=2dt\), \(t:0\to1\).
\[
x^{3/2} = (2t)^{3/2} = 2^{3/2} t^{3/2}
\]
\[
(2-x)^{-1/2} = 2^{-1/2} (1-t)^{-1/2}
\]
So:
\[
I_3 = \int_{t=0}^1 2^{3/2} t^{3/2} \cdot 2^{-1/2} (1-t)^{-1/2} \cdot 2 dt
= \int_0^1 2^{3/2-1/2} t^{3/2} (1-t)^{-1/2} \cdot 2 dt
\]
\[
2^{3/2-1/2}=2^{1}=2
\]
\[
I_3 = \int_0^1 2 t^{3/2}(1-t)^{-1/2} \cdot 2 dt
= 4 \int_0^1 t^{3/2}(1-t)^{-1/2} dt
\]
\[
\int_0^1 t^{a-1}(1-t)^{b-1}dt = \mathrm{B}(a, b)
\]
Here \(a=5/2\), \(b=1/2\):
\[
I_3=4\mathrm{B}(5/2, 1/2)=4 \frac{\Gamma(5/2)\Gamma(1/2)}{\Gamma(3)}
\]
Recall:
\[
\Gamma(5/2) = (3/2)\Gamma(3/2) = (3/2) \cdot (1/2)\sqrt{\pi} = (3/4)\sqrt{\pi}
\]
\[
\Gamma(3) = 2!
\]
Thus,
\[
I_3=4 \cdot \frac{(3/4)\sqrt{\pi}\cdot\sqrt{\pi}}{2} = 4 \cdot \frac{3}{4} \cdot \frac{\pi}{2} = 3 \cdot \frac{\pi}{2} = \frac{3\pi}{2}
\]

---

## Now plug back into \(I = I_1 - I_2 + 0.5 I_3\):

\[
I = \pi - \pi + 0.5 \cdot \frac{3\pi}{2} = 0 + \frac{3\pi}{4} = \frac{3\pi}{4}
\]

---

## Step 3: Numerical approximation (to 10 decimal places):

\[
\frac{3\pi}{4} \approx 2.3561944902
\]

---

## Step 4: JSON Output

```json
{"answer": "\\frac{3\\pi}{4}", "numerical_answer": "2.3561944902"}
```