
To solve the definite integral \(\int_0^1 \left( (1 - x^{25})^{1/20} - (1 - x^{20})^{1/25} \right) \, dx\), we analyze each term separately using the Beta and Gamma functions.

### Step 1: Integral of \((1 - x^{25})^{1/20}\)
Let \(u = x^{25}\), so \(x = u^{1/25}\) and \(dx = \frac{1}{25} u^{-24/25} du\). The integral becomes:
\[
\int_0^1 (1 - x^{25})^{1/20} \, dx = \frac{1}{25} \int_0^1 u^{-24/25} (1 - u)^{1/20} \, du
\]
This matches the Beta function \(B(p, q) = \int_0^1 t^{p-1} (1 - t)^{q-1} \, dt\) with \(p = \frac{1}{25}\) and \(q = \frac{21}{20}\). Using \(B(p, q) = \frac{\Gamma(p)\Gamma(q)}{\Gamma(p+q)}\), we get:
\[
\int_0^1 (1 - x^{25})^{1/20} \, dx = \frac{1}{25} \cdot \frac{\Gamma\left(\frac{1}{25}\right)\Gamma\left(\frac{21}{20}\right)}{\Gamma\left(\frac{1}{25} + \frac{21}{20}\right)}
\]
Simplifying the argument of the denominator Gamma function: \(\frac{1}{25} + \frac{21}{20} = \frac{109}{100}\).

### Step 2: Integral of \((1 - x^{20})^{1/25}\)
Let \(v = x^{20}\), so \(x = v^{1/20}\) and \(dx = \frac{1}{20} v^{-19/20} dv\). The integral becomes:
\[
\int_0^1 (1 - x^{20})^{1/25} \, dx = \frac{1}{20} \int_0^1 v^{-19/20} (1 - v)^{1/25} \, du
\]
This matches the Beta function with \(p = \frac{1}{20}\) and \(q = \frac{26}{25}\). Thus:
\[
\int_0^1 (1 - x^{20})^{1/25} \, dx = \frac{1}{20} \cdot \frac{\Gamma\left(\frac{1}{20}\right)\Gamma\left(\frac{26}{25}\right)}{\Gamma\left(\frac{1}{20} + \frac{26}{25}\right)}
\]
The denominator argument simplifies to \(\frac{1}{20} + \frac{26}{25} = \frac{109}{100}\).

### Step 3: Simplifying with Gamma Function Properties
Using \(\Gamma(z + 1) = z\Gamma(z)\):
- \(\Gamma\left(\frac{21}{20}\right) = \Gamma\left(1 + \frac{1}{20}\right) = \frac{1}{20}\Gamma\left(\frac{1}{20}\right)\)
- \(\Gamma\left(\frac{26}{25}\right) = \Gamma\left(1 + \frac{1}{25}\right) = \frac{1}{25}\Gamma\left(\frac{1}{25}\right)\)

Substituting these into the integrals:
- First integral: \(\frac{1}{25} \cdot \frac{\Gamma\left(\frac{1}{25}\right) \cdot \frac{1}{20}\Gamma\left(\frac{1}{20}\right)}{\Gamma\left(\frac{109}{100}\right)} = \frac{\Gamma\left(\frac{1}{25}\right)\Gamma\left(\frac{1}{20}\right)}{25 \cdot 20 \cdot \Gamma\left(\frac{109}{100}\right)}\)
- Second integral: \(\frac{1}{20} \cdot \frac{\Gamma\left(\frac{1}{20}\right) \cdot \frac{1}{25}\Gamma\left(\frac{1}{25}\right)}{\Gamma\left(\frac{109}{100}\right)} = \frac{\Gamma\left(\frac{1}{20}\right)\Gamma\left(\frac{1}{25}\right)}{20 \cdot 25 \cdot \Gamma\left(\frac{109}{100}\right)}\)

### Step 4: Final Result
The two integrals are equal, so their difference is zero.

### Numerical Approximation
The exact value is \(0\), so the numerical approximation is \(0.0000000000\).

{"answer": "0", "numerical_answer": "0.0000000000"}