# Calculating $\int\sin(101x)\sin(x)^{99}dx$

I'll evaluate this indefinite integral step by step.

## Step 1: Rewrite using power reduction formula

First, let's note that $\sin(x)^{99}$ is an odd power of $\sin(x)$, so I'll use the identity:
$\sin^{2n+1}(x) = \sin(x) \cdot \sin^{2n}(x) = \sin(x) \cdot (1-\cos^2(x))^n$

In our case, $n = 49$, so:
$\sin^{99}(x) = \sin(x) \cdot (1-\cos^2(x))^{49}$

## Step 2: Apply trigonometric identity for product of sines

For the product $\sin(101x)\sin(x)$, I'll use the identity:
$\sin(A)\sin(B) = \frac{1}{2}[\cos(A-B) - \cos(A+B)]$

With $A = 101x$ and $B = x$:
$\sin(101x)\sin(x) = \frac{1}{2}[\cos(100x) - \cos(102x)]$

## Step 3: Rewrite the integral

$\int\sin(101x)\sin(x)^{99}dx = \int\sin(101x)\sin(x) \cdot (1-\cos^2(x))^{49}dx$

$= \frac{1}{2}\int[\cos(100x) - \cos(102x)] \cdot (1-\cos^2(x))^{49}dx$

This is still complex, so let's try a different approach.

## Step 1 (alternative): Use the identity with complex exponentials

Let's use the identity: $\sin(101x)\sin^{99}(x) = \text{Im}(e^{101ix})\sin^{99}(x)$

We can use the binomial expansion of $\sin^{99}(x)$ in terms of complex exponentials:

$\sin(x) = \frac{e^{ix} - e^{-ix}}{2i}$

So $\sin^{99}(x) = \left(\frac{e^{ix} - e^{-ix}}{2i}\right)^{99}$

## Step 2 (better approach): Use the product-to-sum formula directly

Let's use the identity:
$\sin(A)\sin^n(B) = \frac{1}{2^n}\sum_{k=0}^{n}(-1)^{n-k}\binom{n}{k}\sin(A+(n-2k)B)$

In our case, $A = 101x$, $B = x$, and $n = 99$:

$\sin(101x)\sin^{99}(x) = \frac{1}{2^{99}}\sum_{k=0}^{99}(-1)^{99-k}\binom{99}{k}\sin(101x+(99-2k)x)$

$= \frac{1}{2^{99}}\sum_{k=0}^{99}(-1)^{99-k}\binom{99}{k}\sin((200-2k)x)$

## Step 3: Integrate term by term

For each term, we have:
$\int\sin((200-2k)x)dx = -\frac{\cos((200-2k)x)}{200-2k} + C$

So our indefinite integral is:
$\int\sin(101x)\sin^{99}(x)dx = \frac{1}{2^{99}}\sum_{k=0}^{99}(-1)^{99-k}\binom{99}{k}\left(-\frac{\cos((200-2k)x)}{200-2k}\right) + C$

$= -\frac{1}{2^{99}}\sum_{k=0}^{99}(-1)^{99-k}\binom{99}{k}\frac{\cos((200-2k)x)}{200-2k} + C$

Since $(-1)^{99-k} = (-1)^{99}(-1)^{-k} = -(-1)^{-k}$, this simplifies to:

$= \frac{1}{2^{99}}\sum_{k=0}^{99}(-1)^{-k}\binom{99}{k}\frac{\cos((200-2k)x)}{200-2k} + C$

## Final Answer

The indefinite integral is:
$\int\sin(101x)\sin(x)^{99}dx = \frac{1}{2^{99}}\sum_{k=0}^{99}(-1)^{-k}\binom{99}{k}\frac{\cos((200-2k)x)}{200-2k} + C$

Since the original question asked for an indefinite integral (no bounds were specified), this is our final answer. The numerical approximation would depend on the value of x, so without bounds, I cannot provide a single numerical value.

{"answer": "\\frac{1}{2^{99}}\\sum_{k=0}^{99}(-1)^{-k}\\binom{99}{k}\\frac{\\cos((200-2k)x)}{200-2k} + C", "numerical_answer": "N/A"}