Let's proceed step by step:

**Step 1: Find the antiderivative**

Let 
\[
f(x) = x^5 + 5x^4 + 10x^3 + 8x^2 + x
\]

The antiderivative \( F(x) \) is:
\[
\int f(x) \, dx = \int (x^5 + 5x^4 + 10x^3 + 8x^2 + x) \, dx
\]
Integrate term by term:
\[
\int x^5 dx = \frac{x^6}{6}
\]
\[
\int 5x^4 dx = 5\frac{x^5}{5} = x^5
\]
\[
\int 10x^3 dx = 10\frac{x^4}{4} = \frac{5x^4}{2}
\]
\[
\int 8x^2 dx = 8\frac{x^3}{3} = \frac{8x^3}{3}
\]
\[
\int x dx = \frac{x^2}{2}
\]
So
\[
F(x) = \frac{x^6}{6} + x^5 + \frac{5x^4}{2} + \frac{8x^3}{3} + \frac{x^2}{2}
\]

**Step 2: Evaluate at limits**

\[
I = F\left(-\frac{1}{2}\right) - F\left(-\frac{3}{2}\right)
\]

Let's compute each:

---

First, \( x = -\frac{1}{2} \):

- \( x^2 = \frac{1}{4} \)
- \( x^3 = -\frac{1}{8} \)
- \( x^4 = \frac{1}{16} \)
- \( x^5 = -\frac{1}{32} \)
- \( x^6 = \frac{1}{64} \)

Substitute into \( F(x) \):

\[
F\left(-\frac{1}{2}\right) 
= \frac{1}{6}\cdot\frac{1}{64}
+ \left(-\frac{1}{32}\right)
+ \frac{5}{2}\cdot\frac{1}{16}
+ \frac{8}{3}\cdot\left(-\frac{1}{8}\right)
+ \frac{1}{2}\cdot\frac{1}{4}
\]
\[
= \frac{1}{384}
- \frac{1}{32}
+ \frac{5}{32}
- \frac{1}{3}
+ \frac{1}{8}
\]

Now, let's bring all terms to a common denominator (384):

- \( \frac{1}{384} \) 
- \( -\frac{1}{32} = -\frac{12}{384} \)
- \( \frac{5}{32} = \frac{60}{384} \)
- \( -\frac{1}{3} = -\frac{128}{384} \)
- \( \frac{1}{8} = \frac{48}{384} \)

Add them up:
\[
\frac{1 - 12 + 60 - 128 + 48}{384}
= \frac{(1 - 12) + (60 + 48) - 128}{384}
= \frac{(-11) + 108 - 128}{384}
= \frac{97 - 128}{384}
= \frac{-31}{384}
\]

So
\[
F\left(-\frac{1}{2}\right) = -\frac{31}{384}
\]

---

Now \( x = -\frac{3}{2} \):

Compute powers first:

- \( x^2 = \left(\frac{9}{4}\right) \)
- \( x^3 = -\frac{27}{8} \)
- \( x^4 = \frac{81}{16} \)
- \( x^5 = -\frac{243}{32} \)
- \( x^6 = \frac{729}{64} \)

Plug into \( F(x) \):

\[
F\left(-\frac{3}{2}\right) =
\frac{1}{6} \cdot \frac{729}{64}
+ \left(-\frac{243}{32}\right)
+ \frac{5}{2} \cdot \frac{81}{16}
+ \frac{8}{3}\cdot\left(-\frac{27}{8}\right)
+ \frac{1}{2} \cdot \frac{9}{4}
\]

Calculate each term:

- \( \frac{1}{6} \cdot \frac{729}{64} = \frac{729}{384} \)
- \( -\frac{243}{32} \)
- \( \frac{5}{2} \cdot \frac{81}{16} = \frac{5 \times 81}{32} = \frac{405}{32} \)
- \( \frac{8}{3} \cdot -\frac{27}{8} = -\frac{27}{3} = -9 \)
- \( \frac{1}{2} \cdot \frac{9}{4} = \frac{9}{8} \)

Letâ€™s express all terms with denominator 384 (except the -9; write as -\(\frac{3456}{384}\)):

- \( \frac{729}{384} \)
- \( -\frac{243}{32} = -\frac{243 \times 12}{384} = -\frac{2916}{384} \)
- \( \frac{405}{32} = \frac{405 \times 12}{384} = \frac{4860}{384} \)
- \( -9 = -\frac{3456}{384} \)
- \( \frac{9}{8} = \frac{9 \times 48}{384} = \frac{432}{384} \)

Sum all terms:
\[
\frac{729 - 2916 + 4860 - 3456 + 432}{384}
\]
Calculate the numerator step by step:

- \( 729 - 2916 = -2187 \)
- \( -2187 + 4860 = 2673 \)
- \( 2673 - 3456 = -783 \)
- \( -783 + 432 = -351 \)

So:

\[
F\left(-\frac{3}{2}\right) = \frac{-351}{384}
\]

---

**Step 3: Take the difference**

\[
I = F\left(-\frac{1}{2}\right) - F\left(-\frac{3}{2}\right)
= \left(-\frac{31}{384}\right) - \left(-\frac{351}{384}\right)
= \frac{351 - 31}{384}
= \frac{320}{384}
\]
\[
= \frac{5}{6}
\]

**Step 4: Numerical approximation**

\[
\frac{5}{6} = 0.8333333333
\]

**Step 5: JSON format**

```json
{"answer": "\\frac{5}{6}", "numerical_answer": "0.8333333333"}
```