

To solve the definite integral \(\int_0^1 \left( e^{e^x} - e^{e^x - x} \right) dx\), we proceed as follows:

### Step 1: Identify the Antiderivative
Notice that the integrand \(e^{e^x} - e^{e^x - x}\) can be recognized as the derivative of a simpler function. Let \(f(x) = e^{e^x - x}\). We compute its derivative:
\[
f'(x) = \frac{d}{dx} \left( e^{e^x - x} \right) = e^{e^x - x} \cdot \frac{d}{dx} \left( e^x - x \right) = e^{e^x - x} \cdot (e^x - 1).
\]
Expanding this, we get:
\[
f'(x) = e^{e^x - x} \cdot e^x - e^{e^x - x} = e^{(e^x - x) + x} - e^{e^x - x} = e^{e^x} - e^{e^x - x}.
\]
This matches the integrand exactly. Thus, the antiderivative of \(e^{e^x} - e^{e^x - x}\) is \(e^{e^x - x}\).

### Step 2: Evaluate the Definite Integral
Using the Fundamental Theorem of Calculus, we evaluate the antiderivative at the bounds \(x = 1\) and \(x = 0\):
\[
\int_0^1 \left( e^{e^x} - e^{e^x - x} \right) dx = \left[ e^{e^x - x} \right]_0^1.
\]
Substituting the bounds:
\[
\left[ e^{e^x - x} \right]_0^1 = e^{e^1 - 1} - e^{e^0 - 0} = e^{e - 1} - e^1 = e^{e - 1} - e.
\]

### Step 3: Numerical Approximation
To approximate \(e^{e - 1} - e\) numerically:
- \(e \approx 2.718281828459045\)
- \(e - 1 \approx 1.718281828459045\)
- \(e^{e - 1} \approx e^{1.718281828459045} \approx 5.5749415416\)
- Thus, \(e^{e - 1} - e \approx 5.5749415416 - 2.718281828459045 \approx 2.8566597131\).

### Final Answer
The exact value of the integral is \(e^{e - 1} - e\), and its numerical approximation is approximately \(2.8566597131\).

{"answer": "e^{e - 1} - e", "numerical_answer": "2.8566597131"}