Let's solve the integral
\[
\int_{0}^{1} x^{-1/2} \cos\left(2\sqrt{x(1-x)}\right) \, dx.
\]

**Step 1: Substitution**

Let \( x = \sin^2 \theta \), where \( \theta \in [0, \pi/2] \). Then,
- \( dx = 2\sin\theta \cos\theta\, d\theta = \sin(2\theta)\, d\theta \)
- \( x^{-1/2} = (\sin^2\theta)^{-1/2} = \csc \theta \)
- \( \sqrt{x(1-x)} = \sqrt{\sin^2\theta (1-\sin^2\theta)} = \sqrt{\sin^2\theta \cos^2\theta} = \sin\theta \cos\theta = \frac12 \sin 2\theta \)

The limits:
- When \( x=0 \implies \theta = 0 \)
- When \( x=1 \implies \theta = \pi/2 \)

Plug in:
\[
\int_{x=0}^{x=1} x^{-1/2} \cos\left(2\sqrt{x(1-x)}\right) dx =
\int_{\theta=0}^{\theta=\pi/2} \csc\theta \cos\left(\sin 2\theta\right) \sin 2\theta d\theta.
\]
But \(\sin 2\theta = 2\sin\theta\cos\theta\), so:
\[
\sin 2\theta\, d\theta = 2\sin\theta\cos\theta\, d\theta
\]
So,
\[
\csc\theta \cos(\sin 2\theta) \sin 2\theta d\theta =
\csc\theta \cos(\sin 2\theta) \cdot 2\sin\theta\cos\theta d\theta =
2\cos(\sin 2\theta) \cos\theta d\theta
\]

Hence,
\[
I = \int_0^{\pi/2} 2\cos\left(\sin 2\theta\right)\cos\theta\, d\theta
\]

**Step 2: Reduce further**

Let us write:
\[
I = 2\int_0^{\pi/2} \cos(\sin 2\theta)\cos\theta\, d\theta
\]

Let’s utilize the expansion:
\[
\cos(\sin 2\theta) = \sum_{n=0}^\infty \frac{(-1)^n (\sin 2\theta)^{2n}}{(2n)!}
\]
But let’s instead attempt a substitution.

Let’s let \( \phi = 2\theta \), so as \( \theta \) goes from \( 0 \to \pi/2 \), \( \phi \) goes from \( 0 \to \pi \).

Also,
\[
d\theta = \frac{d\phi}{2}
\]
and
\[
\cos\theta = \cos\left(\frac{\phi}{2}\right)
\]

So the integral becomes:
\[
I = 2\int_0^{\pi/2} \cos(\sin 2\theta)\cos\theta\, d\theta = 2\int_0^\pi \cos(\sin \phi)\cos\left(\frac{\phi}{2}\right) \frac{d\phi}{2}
\]
\[
= \int_0^\pi \cos(\sin \phi)\cos\left(\frac{\phi}{2}\right)d\phi
\]

**Step 3: Further simplification**

Recall the identity:
\[
\cos(A)\cos(B) = \frac{1}{2} [\cos(A-B) + \cos(A+B)]
\]

So,
\[
\cos(\sin\phi)\cos\left(\frac{\phi}{2}\right) = \frac{1}{2}\left[ \cos(\sin\phi - \frac{\phi}{2}) + \cos(\sin\phi + \frac{\phi}{2}) \right]
\]

So,
\[
I = \int_0^\pi \cos(\sin\phi)\cos\left(\frac{\phi}{2}\right) d\phi =
\frac{1}{2} \int_0^\pi \left[ \cos(\sin\phi - \frac{\phi}{2}) + \cos(\sin\phi + \frac{\phi}{2}) \right] d\phi
\]

But, integrating either term analytically is challenging.

**Step 4: Series expansion approach**

Alternately, go back to the series expansion:
\[
\cos(2\sqrt{x(1-x)}) = \sum_{n=0}^\infty \frac{(-1)^n (2\sqrt{x(1-x)})^{2n}}{(2n)!}
= \sum_{n=0}^\infty \frac{(-1)^n 2^{2n} [x(1-x)]^n}{(2n)!}
\]
So,
\[
I = \int_0^1 x^{-1/2} \sum_{n=0}^\infty \frac{(-1)^n 2^{2n} [x(1-x)]^n}{(2n)!} dx \\
= \sum_{n=0}^\infty \frac{(-1)^n 2^{2n}}{(2n)!} \int_0^1 x^{-1/2} x^n (1-x)^n dx \\
= \sum_{n=0}^\infty \frac{(-1)^n 2^{2n}}{(2n)!} \int_0^1 x^{n - 1/2} (1-x)^n dx
\]
The integral is a Beta function:
\[
\int_0^1 x^{a-1} (1-x)^{b-1} dx = \mathrm{B}(a,b) = \frac{\Gamma(a)\Gamma(b)}{\Gamma(a+b)}
\]
In our case, \( a = n + 1/2 \), \( b = n + 1 \):

So,
\[
\int_0^1 x^{n-1/2} (1-x)^n dx = \frac{\Gamma(n + 1/2) \Gamma(n + 1)}{\Gamma(2n + 3/2)}
\]
Thus,
\[
I = \sum_{n=0}^\infty \frac{(-1)^n 2^{2n}}{(2n)!} \frac{\Gamma(n + 1/2) \Gamma(n + 1)}{\Gamma(2n + 3/2)}
\]

But \( 2^{2n} = 4^n \), and \( \Gamma(n + 1) = n! \). The result becomes:
\[
I = \sum_{n=0}^\infty \frac{(-1)^n 4^n n! \Gamma(n + 1/2)}{(2n)! \Gamma(2n + 3/2)}
\]

Alternatively, collect all together:
\[
I = \sum_{n=0}^\infty \frac{(-1)^n 4^n \Gamma(n + 1) \Gamma(n + 1/2)}{(2n)! \Gamma(2n + 3/2)}
\]

**Step 5: Closed form?**

Is this sum a known function? Let's try computing the value numerically, but before that, let's check if the integral matches a standard form.

Let’s consult Gradshteyn & Ryzhik 3.944.2 (or similar) for an analogous formula:

\[
\int_0^1 x^{\mu-1} (1-x)^{\nu-1} J_\rho(2a\sqrt{x(1-x)}) dx = \frac{\Gamma(\mu) \Gamma(\nu)}{\Gamma(\mu+\nu)} \left( \frac{a}{2} \right)^\rho J_{\mu+\nu+\rho-1}(a)
\]

But our integrand involves cosine of \(2\sqrt{x(1-x)}\). Recall that \(\cos(z) = \mathrm{Re}\,e^{iz}\), which is a real part of a Bessel function expansion.

But perhaps more directly, let's see that:

\[
\int_0^1 x^{\alpha-1}(1-x)^{\beta-1}\cos[a\sqrt{x(1-x)}] dx = \frac{\Gamma(\alpha)\Gamma(\beta)}{\Gamma(\alpha+\beta)}\, {}_0F_1 \left(; \alpha+\beta; -\frac{a^2}{4} \right)
\]

This formula appears in some integral tables (see Gradshteyn & Ryzhik 3.944.3):

\[
\int_0^1 x^{\mu-1}(1-x)^{\nu-1} \cos\left(2a\sqrt{x(1-x)}\right) dx
= \frac{\Gamma(\mu)\Gamma(\nu)}{\Gamma(\mu+\nu)}\, {}_0F_1\left(; \mu+\nu; -a^2 \right)
\]

With the correspondence:
- \( \mu = 1/2 \) (since \( x^{-1/2} \implies \mu-1 = -1/2 \)), so \( \mu = 1/2 \)
- \( \nu = 1 \)
- \( a = 1 \) (since \( 2a = 2 \implies a = 1 \))

Therefore,
\[
I = \frac{\Gamma(1/2)\Gamma(1)}{\Gamma(3/2)}\, {}_0F_1\left(; 3/2; -1 \right)
\]

Compute the \(\Gamma\) functions:
- \( \Gamma(1/2) = \sqrt{\pi} \)
- \( \Gamma(1) = 1 \)
- \( \Gamma(3/2) = \frac12 \sqrt{\pi} \)

Therefore,
\[
\frac{\sqrt{\pi} \cdot 1}{\frac12 \sqrt{\pi}} = 2
\]
So,

\[
I = 2\, {}_0F_1\left(; 3/2; -1 \right)
\]

**Step 6: Numerical Value**

We need to compute \( 2\, {}_0F_1\left(; 3/2; -1 \right) \).

Recall that
\[
{}_0F_1(; b; z) = \sum_{k=0}^\infty \frac{z^k}{k! (b)_k}
\]
where \( (b)_k \) is the Pochhammer symbol.

Let’s compute this sum up to several terms for \( b = 3/2 \), \( z = -1 \):

- \( k=0 \): \( 1 / (1) = 1 \)
- \( k=1 \): \( (-1) / (1 \cdot (3/2)) = -2/3 \)
- \( k=2 \): \( 1 / (2 \cdot (3/2)(5/2)) = 1/[2 \cdot (3/2) \cdot (5/2)] = 1/[2 \cdot 3/2 \cdot 5/2] = 1/[2 \cdot 1.5 \cdot 2.5] = 1/[2 \cdot 3.75] = 1/7.5 = 0.13333 \) ...(wait, better to compute directly):

\( (3/2)_2 = (3/2) \cdot (5/2) = 15/4 \), so
\( 1/(2! \cdot 15/4) = 1 / (2 \cdot 3.75) = 1/7.5 = 0.133333... \)

But sign alternates:
- \( k=2 \): \( (-1)^2 / (2! (3/2)_2) = 1/(2 \cdot 15/4) = 1/7.5 = 0.133333... \)

- \( k=3 \): \( (-1)^3 / (6 \cdot (3/2)(5/2)(7/2))  \)
\( (3/2)_3 = (3/2)(5/2)(7/2) = 3/2 \cdot 5/2 = 15/4; 15/4 \cdot 7/2 = 105/8 \)
So denominator: \( 6 \cdot 105/8 = 630/8 = 78.75 \)
So term: \( -1 / 78.75 \approx -0.0126984 \)

Fourth term:
- \( k=4 \): \( 1/(24 \cdot (3/2)_4) \), \( (3/2)_4 = (3/2)(5/2)(7/2)(9/2) = (105/8)\cdot(9/2) = 945/16 \), so denominator: \( 24 \cdot 945/16 = 24 \cdot 59.0625 = 1417.5 \)
Thus, term: \( +1 / 1417.5 \approx 0.0007054 \)

Let's sum:

\[
{}_0F_1(; 3/2; -1)  \approx 1 - 0.6666667 + 0.1333333 - 0.0126984 + 0.0007054 \\
= 1 - 0.6666667 = 0.3333333 + 0.1333333 = 0.4666666 - 0.0126984 = 0.4539682 + 0.0007054 = 0.4546736
\]
Now next term (\( k=5 \)):
\( (3/2)_5 = (3/2)(5/2)(7/2)(9/2)(11/2) = 945/16 \cdot 11/2 = 10395/32 = 324.84375 \), denominator: \( 120*324.84375 = 38981.25 \), term: \( -1/38981.25 \approx -0.0000256 \)

New sum: \( 0.4546736 - 0.0000256 = 0.454648 \)

Thus, the value converges rapidly to about 0.454648.

Multiply by 2: \( 0.454648 \cdot 2 = 0.909296 \)

But let's do a more precise evaluation.

Alternatively, from known resources,
\( {}_0F_1(;3/2;-1) = \frac{\sqrt{\pi}}{2} J_{-1/2}(2) \)
But \( J_{-\nu}(z) = (-1)^\nu J_\nu(z) \), and for half-integer orders,
\[
J_{-1/2}(z) = \sqrt{\frac{2}{\pi z}} \cos z
\]
And so,
\[
{}_0F_1(;3/2;-1) = \frac{\sqrt{\pi}}{2} \sqrt{\frac{2}{\pi 2}}\cos(2) = \frac{\sqrt{\pi}}{2} \cdot \sqrt{\frac{1}{\pi}} \cos(2) \\
= \frac{\sqrt{\pi}}{2\sqrt{\pi}}\cos(2) = \frac{1}{2}\cos(2)
\]
But this gives a numerical mismatch from before. Let's check carefully.

Let’s recall:

From G&R 9.131.1:

\[
{}_0F_1(; \alpha+1; -z^2/4) = \Gamma(\alpha+1)(z/2)^{-\alpha} J_\alpha(z)
\]
In our case,
- \( \alpha+1 = 3/2 \implies \alpha = 1/2 \)
- \( z^2/4 = 1 \implies z = 2 \)

So

\[
{}_0F_1(; 3/2; -1) = \Gamma(3/2)\cdot (2/2)^{-1/2} J_{1/2}(2)
= \frac{1}{2}\sqrt{\pi} \cdot 1^{-1/2} J_{1/2}(2)
= \frac{1}{2}\sqrt{\pi} J_{1/2}(2)
\]

Recall \( J_{1/2}(z) = \sqrt{\frac{2}{\pi z}} \sin z \).

So

\[
J_{1/2}(2) = \sqrt{\frac{2}{\pi 2}}\sin(2) = \sqrt{\frac{1}{\pi}}\sin(2)
\]

Therefore,

\[
{}_0F_1(; 3/2; -1) = \frac{1}{2}\sqrt{\pi} \cdot \sqrt{\frac{1}{\pi}}\sin(2)
= \frac{1}{2}\sin(2)
\]
Therefore,

\[
I = 2 \cdot {}_0F_1(;3/2;-1) = 2 \cdot \frac{1}{2}\sin(2) = \sin(2)
\]

**Step 7: Final answer**

Thus, the exact answer is \( \boxed{\sin(2)} \).

Now, numerically:
\[
\sin(2) \approx 0.9092974268
\]

**Step 8: Format as requested in JSON**

```json
{"answer": "\\sin(2)", "numerical_answer": "0.9092974268"}
```