We want to evaluate

  I = ∫₀^(2π) |1 + 2 sin x| dx.

Step 1. Find the zeros of the integrand
We need to know where the expression inside the absolute value changes sign. Solve:
  1 + 2 sin x = 0 ⟹ sin x = –1/2.
In the interval [0, 2π] the solutions are:
  x = 7π/6 and x = 11π/6.

Step 2. Split the integral
Examine the sign of 1 + 2 sin x in the various subintervals:
• For x in [0, 7π/6]: At x = 0, sin0 = 0 so 1 + 2·0 = 1 > 0. Thus, the integrand is nonnegative.
• For x in [7π/6, 11π/6]: Taking x = 3π/2 gives sin(3π/2) = –1, so 1 + 2(–1) = –1 < 0.
• For x in [11π/6, 2π]: At x = 2π, sin(2π) = 0 so 1 + 2·0 = 1 > 0.
Thus, we break the integral into three parts:
  I = ∫₀^(7π/6) (1 + 2 sin x) dx + ∫_(7π/6)^(11π/6) –(1 + 2 sin x) dx + ∫_(11π/6)^(2π) (1 + 2 sin x) dx.

Step 3. Find the antiderivative
The antiderivative of 1 + 2 sin x is:
  A(x) = ∫ (1 + 2 sin x) dx = x – 2 cos x + C.

Step 4. Evaluate each part

• Part 1: I₁ = ∫₀^(7π/6) (1 + 2 sin x) dx
  I₁ = [A(7π/6) – A(0)]
   = [(7π/6) – 2 cos(7π/6)] – [0 – 2 cos 0]
  Note: cos(7π/6) = –√3/2 and cos 0 = 1, so
  I₁ = 7π/6 – 2(–√3/2) + 2(1) = 7π/6 + √3 + 2.

• Part 2: I₂ = ∫_(7π/6)^(11π/6) –(1 + 2 sin x) dx
  I₂ = –[A(11π/6) – A(7π/6)]
   = –{ [11π/6 – 2 cos(11π/6)] – [7π/6 – 2 cos(7π/6)] }
   = –{ (11π/6 – 7π/6) – 2[cos(11π/6) – cos(7π/6)] }
   = –{ (4π/6) – 2[cos(11π/6) – cos(7π/6)] }
  Simplify: 4π/6 = 2π/3.
  Recall: cos(11π/6) = √3/2 and cos(7π/6) = –√3/2, so
  cos(11π/6) – cos(7π/6) = (√3/2 – (–√3/2)) = √3.
  Thus, I₂ = –(2π/3 – 2√3) = 2√3 – 2π/3.

• Part 3: I₃ = ∫_(11π/6)^(2π) (1 + 2 sin x) dx
  I₃ = A(2π) – A(11π/6)
   = [2π – 2 cos 2π] – [11π/6 – 2 cos(11π/6)]
  Note: cos 2π = 1 and cos(11π/6) = √3/2, so
  I₃ = 2π – 2(1) – 11π/6 + 2(√3/2)
   = 2π – 2 – 11π/6 + √3.
  Write 2π as 12π/6:
  I₃ = (12π/6 – 11π/6) – 2 + √3 = π/6 – 2 + √3.

Step 5. Sum the parts
  I = I₁ + I₂ + I₃
  = (7π/6 + √3 + 2) + (2√3 – 2π/3) + (π/6 – 2 + √3).

Combine like terms:
• π terms: 7π/6 + (–2π/3) + π/6 = (7π/6 + π/6) – 2π/3 = (8π/6) – 2π/3 = (4π/3) – (2π/3) = 2π/3.
• Constant terms: 2 – 2 = 0.
• √3 terms: √3 + 2√3 + √3 = 4√3.

Thus, the integral is:
  I = 2π/3 + 4√3.

Step 6. Numerical approximation
Compute:
  2π/3 ≈ 2 × 3.141592653589793 / 3 ≈ 2.0943951023931953,
  4√3 ≈ 4 × 1.7320508075688772 ≈ 6.928203230275509.
Then:
  I ≈ 2.0943951023931953 + 6.928203230275509 ≈ 9.022598332668705.
Rounded to 10 decimal places, I ≈ 9.0225983327.

Final Output in JSON format:

{"answer": "$\\frac{2\\pi}{3}+4\\sqrt{3}$", "numerical_answer": "9.0225983327"}