Let's solve the integral:
\[
I = \int_{-4}^{4} e^{|x|}\cdot\{x\}\;dx
\]
where \(\{x\}\) is the fractional part of \(x\): \(\{x\} = x - \lfloor x \rfloor\).

---

### Step 1: Analyze Symmetry

Since \(\{x\}\) is not an even or odd function, let's check if we can express the integral in terms of simpler intervals.

Note that for any integer \(n\):

- Over \([n, n+1)\), \(\{x\} = x - n\)
- For \(x<0\), we can write \(\{x\} = x - \lceil x\rceil + 1\)

But perhaps more simply, we can split the interval \([-4,0)\) and \([0,4]\):

#### For \(x \in [0,4]\):

- \(|x| = x\)
- \(\{x\} = x - \lfloor x \rfloor\)

#### For \(x \in [-4,0)\):

- \(|x| = -x\)
- For negative \(x\), \(\{x\} = x - \lfloor x \rfloor\), but for negative \(x\), \(\lfloor x \rfloor\) is one less than \(x\) if \(x\) is not integer.

But specifically, for \(x \in [-4,0)\):

Let \(x=-y, y \in (0,4]\)

Then \(x \in [-4,0) \implies y \in (0,4]\)

Let us perform substitution \(x = -y,\, y \in (0,4]\):

For \(x = -y\):

- \(|x| = y\)
- \(\{x\} = x - \lfloor x \rfloor\)

Let's compute \(\{x\}\) for \(x=-y, \; y\in(0,4]\):

\[
\{x\} = x - \lfloor x \rfloor = -y - \lfloor -y \rfloor
\]

But \(\lfloor -y \rfloor = -\lceil y \rceil\), since floor of negative is minus ceiling. More precisely,

- If \(y\) is not integer, \(\lfloor -y \rfloor = -\lceil y \rceil\), and
- \(\{x\} = -y + \lceil y \rceil\)
- For \(y \in (k, k+1],\; k=0,1,2,3\), \(\lceil y \rceil = k+1\)
- So \(\{x\} = -y + k + 1\) for \(y \in (k, k+1]\)

---

### Step 2: Split and Express the Integral

Let us write
\[
I = \int_{-4}^0 e^{|x|}\{x\}\;dx + \int_0^4 e^{|x|}\{x\}\;dx
\]

#### For \(x \in [-4,0)\):

Let \(x = -y,\; y \in (0,4]\):

\[
\begin{align*}
I_1 &= \int_{-4}^0 e^{|x|}\{x\}\;dx \\
    &= \int_{y=4}^{y=0} e^{y} \left[ -y + \lceil y \rceil \right] (-dy) \\
    &= \int_{0}^{4} e^{y} \left[ y - \lceil y \rceil \right] dy
\end{align*}
\]

#### For \(x \in [0,4)\):

Write as sum over intervals:

\[
I_2 = \int_0^4 e^{x} \{x\}\,dx = \sum_{k=0}^{3} \int_{x=k}^{k+1} e^x (x-k) dx
\]

Similarly,
\[
I_1 = \int_0^4 e^{y}(y - \lceil y\rceil) dy = \sum_{k=0}^{3} \int_{y=k}^{k+1} e^y (y - (k+1)) dy
\]

Therefore,

\[
I = \sum_{k=0}^3 \left[ \int_{k}^{k+1} e^{x} (x-k) dx + \int_{k}^{k+1} e^{x} (x - (k+1)) dx \right]
\]

But:
\[
(x-k) + (x - (k+1)) = 2x - (2k+1)
\]

So for each \(k\), over \(x \in [k, k+1]\):
\[
I = \sum_{k=0}^3 \int_{x = k}^{k+1} e^{x}(2x - (2k+1))dx
\]

---

### Step 3: Compute the Integral

We now need:
\[
I = \sum_{k=0}^3 \int_{k}^{k+1} e^{x} (2x - (2k+1))dx
\]

Let's compute the indefinite integral:
\[
\int e^{x}(2x - A) dx
\]
Let \(A = 2k+1\).

Let us use integration by parts:
Let \(u = 2x - A\), \(dv = e^{x} dx\)
\[
du = 2 dx,\quad v = e^{x}
\]
Therefore,
\[
\int e^{x}(2x-A) dx = (2x-A)e^{x} - \int 2 e^{x} dx = (2x-A)e^{x} - 2e^{x} + C
\]

So over \([k, k+1]\):

\[
J(k) = \int_{k}^{k+1} e^{x}(2x-(2k+1))dx = \left[ (2x - (2k+1))e^{x} - 2e^{x} \right]_{x=k}^{x=k+1}
\]

Evaluate at endpoints:

\[
J(k) = \left\{ (2(k+1) - (2k+1))e^{k+1} - 2e^{k+1} \right\} - \left\{ (2k - (2k+1))e^{k} - 2e^{k} \right\}
\]

\[
2(k+1) - (2k+1) = 2k + 2 - 2k - 1 = 1
\]
So at \(x=k+1\):
\[
(2(k+1)-(2k+1))e^{k+1} - 2e^{k+1} = (1)e^{k+1} - 2e^{k+1} = -e^{k+1}
\]
At \(x=k\):
\[
2k-(2k+1) = -1
\]
So:
\[
(-1)e^k - 2e^k = -e^k - 2e^k = -3e^k
\]

Therefore,
\[
J(k) = [-e^{k+1} - (-3e^k)] = -e^{k+1} + 3e^k
\]

---

### Step 4: Express the Sum

So the total:
\[
I = \sum_{k=0}^3 J(k) = \sum_{k=0}^3 (3e^k - e^{k+1}) = 3\sum_{k=0}^3 e^k - \sum_{k=0}^3 e^{k+1}
\]

But \(\sum_{k=0}^3 e^k = e^0 + e^1 + e^2 + e^3\)

\(\sum_{k=0}^3 e^{k+1} = e^1 + e^2 + e^3 + e^4 = \sum_{k=1}^4 e^k\)

So,

\[
I = 3(e^0 + e^1 + e^2 + e^3) - (e^1 + e^2 + e^3 + e^4)
\]
\[
= 3e^0 + 3e^1 + 3e^2 + 3e^3 - e^1 - e^2 - e^3 - e^4
\]
\[
= 3e^0 + (3e^1 - e^1) + (3e^2 - e^2) + (3e^3 - e^3) - e^4
\]
\[
= 3e^0 + 2e^1 + 2e^2 + 2e^3 - e^4
\]
Recalling that \(e^0 = 1\):

\[
\boxed{
I = 3 + 2e^1 + 2e^2 + 2e^3 - e^4
}
\]

---

### Step 5: Numerical Approximation

To 10 decimal places, calculate:
- \(e^1 \approx 2.7182818285\)
- \(e^2 \approx 7.3890560989\)
- \(e^3 \approx 20.0855369232\)
- \(e^4 \approx 54.5981500331\)

Plug in:
\[
I = 3 + 2\cdot 2.7182818285 + 2\cdot 7.3890560989 + 2\cdot 20.0855369232 - 54.5981500331
\]
\[
= 3 + 5.4365636570 + 14.7781121978 + 40.1710738464 - 54.5981500331
\]
\[
= (3 + 5.4365636570 + 14.7781121978 + 40.1710738464) - 54.5981500331
\]
\[
= 63.3857507012 - 54.5981500331
\]
\[
= 8.7876006681
\]

Rounded to 10 decimal places:

\[
\boxed{8.7876006681}
\]

---

### Step 6: Final JSON Output

```json
{"answer": "3 + 2e^{1} + 2e^{2} + 2e^{3} - e^{4}", "numerical_answer": "8.7876006681"}
```