To compute the definite integral \(\int_0^1 (x-1)^2(x+1)^2(x^2+1)^2(x^4+1)^2 \, dx\), we can simplify the integrand first.

### Step 1: Simplify the Integrand
Notice that:
\[
(x-1)^2(x+1)^2 = [(x-1)(x+1)]^2 = (x^2 - 1)^2
\]
So the integrand becomes:
\[
(x^2 - 1)^2 (x^2 + 1)^2 (x^4 + 1)^2
\]
Next, observe that:
\[
(x^2 - 1)(x^2 + 1) = x^4 - 1
\]
Thus:
\[
(x^2 - 1)^2 (x^2 + 1)^2 = (x^4 - 1)^2
\]
Now the integrand is:
\[
(x^4 - 1)^2 (x^4 + 1)^2 = [(x^4 - 1)(x^4 + 1)]^2 = (x^8 - 1)^2
\]
So the integral simplifies to:
\[
\int_0^1 (x^8 - 1)^2 \, dx
\]

### Step 2: Expand and Integrate
Expand \((x^8 - 1)^2\):
\[
(x^8 - 1)^2 = x^{16} - 2x^8 + 1
\]
Now integrate term by term:
\[
\int_0^1 (x^{16} - 2x^8 + 1) \, dx = \left[ \frac{x^{17}}{17} - \frac{2x^9}{9} + x \right]_0^1
\]
Evaluate at the bounds:
\[
\left( \frac{1}{17} - \frac{2}{9} + 1 \right) - (0 - 0 + 0) = \frac{1}{17} - \frac{2}{9} + 1
\]

### Step 3: Compute the Exact Value
Combine the terms:
\[
1 + \frac{1}{17} - \frac{2}{9} = \frac{153}{153} + \frac{9}{153} - \frac{34}{153} = \frac{153 + 9 - 34}{153} = \frac{128}{153}
\]
So the exact value is:
\[
\frac{128}{153}
\]

### Step 4: Numerical Approximation
Compute the numerical value of \(\frac{128}{153}\):
\[
\frac{128}{153} \approx 0.8366013072
\]

### Final Answer
```json
{"answer": "\\frac{128}{153}", "numerical_answer": "0.8366013072"}
```