<think>
Okay, let's tackle this integral step by step. The integral given is ∫₁^∞ x(x² - 1²)^{2 - 3/2} e^{-0.25x²} H_{4}(0.5x) dx. First, I need to simplify the exponents and understand each part of the integrand.

Starting with the term (x² - 1)^{2 - 3/2}. Let me compute 2 - 3/2. That's 2 - 3/2 = 1/2. So this term becomes (x² - 1)^{1/2}, which is the square root of (x² - 1). So the integrand simplifies to x * sqrt(x² - 1) * e^{-0.25x²} multiplied by the Hermite polynomial H₄(0.5x).

Next, I need to recall the form of the Hermite polynomial H₄(y). The Hermite polynomials are given by H_n(y) = (-1)^n e^{y²} d^n/dy^n e^{-y²}. For n=4, H₄(y) = 16y⁴ - 48y² + 12. Let me confirm that. Wait, the explicit formula for H₄(y) is indeed 16y⁴ - 48y² + 12. So substituting y = 0.5x, H₄(0.5x) = 16*(0.5x)^4 - 48*(0.5x)^2 + 12. Let me compute each term:

(0.5x)^4 = (x^4)/16, so 16*(x^4/16) = x^4. Then, (0.5x)^2 = x²/4, so 48*(x²/4) = 12x². Wait, but the coefficient is -48? Wait, H₄(y) is 16y⁴ - 48y² + 12? Wait, maybe I made a mistake here. Let me check the standard Hermite polynomials. H₀(y)=1, H₁(y)=2y, H₂(y)=4y² - 2, H₃(y)=8y³ - 12y, H₄(y)=16y⁴ - 48y² + 12. Yes, that's correct. So H₄(y) = 16y⁴ - 48y² + 12. So substituting y = 0.5x, we get:

H₄(0.5x) = 16*(0.5x)^4 - 48*(0.5x)^2 + 12 = 16*(x^4/16) - 48*(x²/4) + 12 = x⁴ - 12x² + 12.

So the integrand becomes x*sqrt(x² - 1)*e^{-0.25x²}*(x⁴ - 12x² + 12).

Now, the integral is from x=1 to infinity. The presence of sqrt(x² - 1) suggests a substitution to simplify the integral. Let me consider substituting t = x² - 1. Then dt/dx = 2x, so x dx = dt/2. But let's see if that helps. Alternatively, maybe a substitution like x = cosh(u) because sqrt(x² -1) is similar to sinh(u) when x = cosh(u), but since x starts at 1, which is cosh(0), but integrating to infinity, that might be a hyperbolic substitution. Alternatively, maybe a substitution t = x². Let's try that.

Let t = x². Then dt = 2x dx, so x dx = dt/2. The limits when x=1, t=1, and as x approaches infinity, t approaches infinity. Then sqrt(x² -1) becomes sqrt(t -1). The integral becomes:

∫₁^∞ sqrt(t -1) * e^{-0.25t} * (t² - 12t + 12) * (x dx) = ∫₁^∞ sqrt(t -1) * e^{-0.25t} * (t² - 12t + 12) * (dt/2).

Wait, but the original integrand after substitution would be x*sqrt(x² -1)*e^{-0.25x²}*(x⁴ -12x² +12) dx. Since x⁴ = t², x² = t, so x⁴ -12x² +12 = t² -12t +12. So yes, substituting t = x², the integral becomes (1/2) ∫₁^∞ sqrt(t -1) e^{-0.25t} (t² -12t +12) dt.

Hmm, but integrating this might still complicated. Alternatively, perhaps another substitution. Let me think. The term sqrt(t -1) suggests substituting u = t -1, so t = u +1, dt = du. Then the integral becomes (1/2) ∫₀^∞ sqrt(u) e^{-0.25(u +1)} ( (u +1)^2 -12(u +1) +12 ) du.

Expanding the polynomial inside:

(u +1)^2 -12(u +1) +12 = u² + 2u +1 -12u -12 +12 = u² -10u +1.

So the integral is (1/2) e^{-0.25} ∫₀^∞ sqrt(u) e^{-0.25u} (u² -10u +1) du.

Now, this looks like a combination of integrals of the form ∫₀^∞ u^{k} e^{-a u} du, which is Gamma functions. Specifically, Gamma(n) = ∫₀^∞ u^{n-1} e^{-a u} du = a^{-n} Γ(n). But here, the exponent is sqrt(u) which is u^{1/2}, multiplied by u², u, and constants. Let's break it into three integrals:

Integral = (1/2) e^{-0.25} [ ∫₀^∞ u^{1/2} e^{-0.25u} u² du -10 ∫₀^∞ u^{1/2} e^{-0.25u} u du + ∫₀^∞ u^{1/2} e^{-0.25u} du ]

Simplify each term:

First integral: u^{1/2 + 2} = u^{5/2} → ∫ u^{5/2} e^{-0.25u} du

Second integral: u^{1/2 +1} = u^{3/2} → ∫ u^{3/2} e^{-0.25u} du

Third integral: u^{1/2} → ∫ u^{1/2} e^{-0.25u} du

Each of these can be expressed using the Gamma function. Recall that ∫₀^∞ u^{k} e^{-a u} du = a^{-(k+1)} Γ(k+1). Wait, more precisely, the integral is Γ(k+1)/a^{k+1} when the integral is ∫₀^∞ u^k e^{-a u} du. But here, the exponent is e^{-0.25u}, so a = 0.25.

So for the first integral: k = 5/2. Then Γ(5/2 +1) = Γ(7/2) = (5/2)(3/2)(1/2)√π) = (15/8)√π. Similarly, the integral is Γ(7/2) / (0.25)^{7/2}.

Wait, let me compute each term step by step.

First integral: ∫ u^{5/2} e^{-0.25u} du from 0 to ∞ = Γ(7/2) / (0.25)^{7/2}

Second integral: ∫ u^{3/2} e^{-0.25u} du = Γ(5/2) / (0.25)^{5/2}

Third integral: ∫ u^{1/2} e^{-0.25u} du = Γ(3/2) / (0.25)^{3/2}

Now, let's compute each Gamma function:

Γ(7/2) = (5/2)(3/2)(1/2)√π) = (15/8)√π

Γ(5/2) = (3/2)(1/2)√π) = (3/4)√π

Γ(3/2) = (1/2)√π

So substituting these into the integrals:

First term: (15/8)√π / (0.25)^{7/2}

Second term: (3/4)√π / (0.25)^{5/2}

Third term: (1/2)√π / (0.25)^{3/2}

Now, compute the denominators. 0.25 is 1/4, so (1/4)^{n} where n is 7/2, 5/2, 3/2.

(1/4)^{7/2} = (4^{-1})^{7/2} = 4^{-7/2} = (2^2)^{-7/2} = 2^{-7} = 1/128

Wait, but 4^{7/2} = (4^{1/2})^7 = 2^7 = 128, so 1/4^{7/2} = 1/128.

Similarly, 1/4^{5/2} = 1/(2^5) = 1/32

1/4^{3/2} = 1/(2^3) = 1/8

Wait, let me confirm:

For (1/4)^{7/2} = (4)^{-7/2} = (2^2)^{-7/2} = 2^{-7} = 1/128. Yes.

Similarly, (1/4)^{5/2} = 2^{-5} = 1/32

(1/4)^{3/2} = 2^{-3} = 1/8

So substituting back:

First term: (15/8)√π / (1/128) = (15/8) * 128 √π = 15 * 16 √π = 240√π

Second term: (3/4)√π / (1/32) = (3/4)*32 √π = 24√π

Third term: (1/2)√π / (1/8) = (1/2)*8 √π = 4√π

Putting it all together:

Integral = (1/2) e^{-0.25} [ 240√π -10*24√π + 4√π ]

Compute inside the brackets:

240√π - 240√π +4√π = 4√π

So Integral = (1/2) e^{-0.25} *4√π = 2 e^{-0.25} √π

Simplify further: 2√π e^{-1/4}

So the exact answer is 2√π e^{-1/4}

Now, let's compute the numerical approximation.

First, compute √π ≈ 1.7724538509

e^{-1/4} ≈ e^{-0.25} ≈ 0.7788007830

Multiply them: 1.7724538509 * 0.7788007830 ≈ 1.380388447

Multiply by 2: 2 * 1.380388447 ≈ 2.760776894

Rounded to 10 decimal places: 2.7607768941

Wait, let me check the multiplication again.

√π ≈ 1.7724538509

e^{-0.25} ≈ 0.778800783071

Multiply these two: 1.7724538509 * 0.778800783071

Let me compute this step by step:

1.7724538509 * 0.778800783071

First, 1 * 0.7788 = 0.7788

0.7 * 0.7788 = 0.54516

0.07 * 0.7788 = 0.054516

0.0024 * 0.7788 ≈ 0.00186912

Adding up: 0.7788 + 0.54516 = 1.32396; +0.054516 = 1.378476; +0.00186912 ≈ 1.38034512

But this is approximate. Let me use a calculator:

1.7724538509 * 0.778800783071

Using a more precise calculation:

1.7724538509 × 0.778800783071 ≈

Let me use calculator steps:

1.7724538509 × 0.778800783071 ≈

First, 1.7724538509 × 0.7 = 1.24071769563

1.7724538509 × 0.07 = 0.12407176956

1.7724538509 × 0.008 = 0.0141796308

1.7724538509 × 0.0008 = 0.001417963

1.7724538509 × 0.000000783071 ≈ approx 0.000001388

Adding all these up:

1.24071769563 + 0.12407176956 = 1.36478946519

+0.0141796308 = 1.37896909599

+0.001417963 = 1.38038705899

+0.000001388 ≈ 1.38038844699

So approximately 1.380388447. Then multiply by 2: 2 * 1.380388447 ≈ 2.760776894

Rounded to 10 decimal places: 2.7607768940

So the numerical approximation is approximately 2.7607768940.

Therefore, the exact answer is 2√π e^{-1/4}, and the numerical value is approximately 2.7607768940.
</think>

{"answer": "2\\sqrt{\\pi} e^{-\\frac{1}{4}}", "numerical_answer": 2.7607768940}