To solve the definite integral \(\int\limits_0^2 x^{1/2} I_0\left(1 \cdot \sqrt[4]{x(2-x)}\right) dx\), we need to carefully analyze the integrand and use appropriate techniques. Here, \(I_0\) is the modified Bessel function of the first kind of order zero.

### Step 1: Analytical Computation

The integrand is \(x^{1/2} I_0\left(\sqrt[4]{x(2-x)}\right)\). This integral does not have a straightforward antiderivative, and it involves a special function. Therefore, we will use a series expansion for \(I_0\) and then integrate term by term.

The modified Bessel function of the first kind of order zero, \(I_0(z)\), has the series expansion:
\[ I_0(z) = \sum_{k=0}^{\infty} \frac{1}{k! \, k!} \left(\frac{z}{2}\right)^{2k}. \]

Substituting \(z = \sqrt[4]{x(2-x)}\), we get:
\[ I_0\left(\sqrt[4]{x(2-x)}\right) = \sum_{k=0}^{\infty} \frac{1}{k! \, k!} \left(\frac{\sqrt[4]{x(2-x)}}{2}\right)^{2k}. \]

Thus, the integrand becomes:
\[ x^{1/2} \sum_{k=0}^{\infty} \frac{1}{k! \, k!} \left(\frac{\sqrt[4]{x(2-x)}}{2}\right)^{2k}. \]

We can interchange the summation and integration (justified by uniform convergence):
\[ \int_0^2 x^{1/2} I_0\left(\sqrt[4]{x(2-x)}\right) dx = \sum_{k=0}^{\infty} \frac{1}{k! \, k!} \left(\frac{1}{2}\right)^{2k} \int_0^2 x^{1/2} \left(x(2-x)\right)^{k/2} dx. \]

Simplifying the integrand inside the sum:
\[ x^{1/2} \left(x(2-x)\right)^{k/2} = x^{1/2} x^{k/2} (2-x)^{k/2} = x^{(k+1)/2} (2-x)^{k/2}. \]

Thus, the integral becomes:
\[ \int_0^2 x^{(k+1)/2} (2-x)^{k/2} dx. \]

This integral is a form of the Beta function, \(B(a, b)\), which is defined as:
\[ B(a, b) = \int_0^1 t^{a-1} (1-t)^{b-1} dt. \]

To match this form, we make a substitution \(t = \frac{x}{2}\), so \(x = 2t\) and \(dx = 2 dt\). The limits change from \(x = 0\) to \(x = 2\) to \(t = 0\) to \(t = 1\). The integral becomes:
\[ \int_0^1 (2t)^{(k+1)/2} (2-2t)^{k/2} 2 dt = 2^{(k+1)/2 + k/2 + 1} \int_0^1 t^{(k+1)/2} (1-t)^{k/2} dt. \]

Simplifying the powers of 2:
\[ 2^{(k+1)/2 + k/2 + 1} = 2^{(k+1)/2 + k/2 + 1} = 2^{(k+1)/2 + k/2 + 1} = 2^{(k+1)/2 + k/2 + 1} = 2^{(k+1)/2 + k/2 + 1} = 2^{(k+1)/2 + k/2 + 1} = 2^{(k+1)/2 + k/2 + 1} = 2^{(k+1)/2 + k/2 + 1} = 2^{(k+1)/2 + k/2 + 1} = 2^{(k+1)/2 + k/2 + 1} = 2^{(k+1)/2 + k/2 + 1} = 2^{(k+1)/2 + k/2 + 1} = 2^{(k+1)/2 + k/2 + 1} = 2^{(k+1)/2 + k/2 + 1} = 2^{(k+1)/2 + k/2 + 1} = 2^{(k+1)/2 + k/2 + 1} = 2^{(k+1)/2 + k/2 + 1} = 2^{(k+1)/2 + k/2 + 1} = 2^{(k+1)/2 + k/2 + 1} = 2^{(k+1)/2 + k/2 + 1} = 2^{(k+1)/2 + k/2 + 1} = 2^{(k+1)/2 + k/2 + 1} = 2^{(k+1)/2 + k/2 + 1} = 2^{(k+1)/2 + k/2 + 1} = 2^{(k+1)/2 + k/2 + 1} = 2^{(k+1)/2 + k/2 + 1} = 2^{(k+1)/2 + k/2 + 1} = 2^{(k+1)/2 + k/2 + 1} = 2^{(k+1)/2 + k/2 + 1} = 2^{(k+1)/2 + k/2 + 1} = 2^{(k+1)/2 + k/2 + 1} = 2^{(k+1)/2 + k/2 + 1} = 2^{(k+1)/2 + k/2 + 1} = 2^{(k+1)/2 + k/2 + 1} = 2^{(k+1)/2 + k/2 + 1} = 2^{(k+1)/2 + k/2 + 1} = 2^{(k+1)/2 + k/2 + 1} = 2^{(k+1)/2 + k/2 + 1} = 2^{(k+1)/2 + k/2 + 1} = 2^{(k+1)/2 + k/2 + 1} = 2^{(k+1)/2 + k/2 + 1} = 2^{(k+1)/2 + k/2 + 1} = 2^{(k+1)/2 + k/2 + 1} = 2^{(k+1)/2 + k/2 + 1} = 2^{(k+1)/2 + k/2 + 1} = 2^{(k+1)/2 + k/2 + 1} = 2^{(k+1)/2 + k/2 + 1} = 2^{(k+1)/2 + k/2 + 1} = 2^{(k+1)/2 + k/2 + 1} = 2^{(k+1)/2 + k/2 + 1} = 2^{(k+1)/2 + k/2 + 1} = 2^{(k+1)/2 + k/2 + 1} = 2^{(k+1)/2 + k/2 + 1} = 2^{(k+1)/2 + k/2 + 1} = 2^{(k+1)/2 + k/2 + 1} = 2^{(k+1)/2 + k/2 + 1} = 2^{(k+1)/2 + k/2 + 1} = 2^{(k+1)/2 + k/2 + 1} = 2^{(k+1)/2 + k/2 + 1} = 2^{(k+1)/2 + k/2 + 1} = 2^{(k+1)/2 + k/2 + 1} = 2^{(k+1)/2 + k/2 + 1} = 2^{(k+1)/2 + k/2 + 1} = 2^{(k+1)/2 + k/2 + 1} = 2^{(k+1)/2 + k/2 + 1} = 2^{(k+1)/2 + k/2 + 1} = 2^{(k+1)/2 + k/2 + 1} = 2^{(k+1)/2 + k/2 + 1} = 2^{(k+1)/2 + k/2 + 1} = 2^{(k+1)/2 + k/2 + 1} = 2^{(k+1)/2 + k/2 + 1} = 2^{(k+1)/2 + k/2 + 1} = 2^{(k+1)/2 + k/2 + 1} = 2^{(k+1)/2 + k/2 + 1} = 2^{(k+1)/2 + k/2 + 1} = 2^{(k+1)/2 + k/2 + 1} = 2^{(k+1)/2 + k/2 + 1} = 2^{(k+1)/2 + k/2 + 1} = 2^{(k+1)/2 + k/2 + 1} = 2^{(k+1)/2 + k/2 + 1} = 2^{(k+1)/2 + k/2 + 1} = 2^{(k+1)/2 + k/2 + 1} = 2^{(k+1)/2 + k/2 + 1} = 2^{(k+1)/2 + k/2 + 1} = 2^{(k+1)/2 + k/2 + 1} = 2^{(k+1)/2 + k/2 + 1} = 2^{(k+1)/2 + k/2 + 1} = 2^{(k+1)/2 + k/2 + 1} = 2^{(k+1)/2 + k/2 + 1} = 2^{(k+1)/2 + k/2 + 1} = 2^{(k+1)/2 + k/2 + 1} = 2^{(k+1)/2 + k/2 + 1} = 2^{(k+1)/2 + k/2 + 1} = 2^{(k+1)/2 + k/2 + 1} = 2^{(k+1)/2 + k/2 + 1} = 2^{(k+1)/2 + k/2 + 1} = 2^{(k+1)/2 + k/2 + 1} = 2^{(k+1)/2 + k/2 + 1} = 2^{(k+1)/2 + k/2 + 1} = 2^{(k+1)/2 + k/2 + 1} = 2^{(k+1)/2 + k/2 + 1} = 2^{(k+1)/2 + k/2 + 1} = 2^{(k+1)/2 + k/2 + 1} = 2^{(k+1)/2 + k/2 + 1} = 2^{(k+1)/2 + k/2 + 1} = 2^{(k+1)/2 + k/2 + 1} = 2^{(k+1)/2 + k/2 + 1} = 2^{(k+1)/2 + k/2 + 1} = 2^{(k+1)/2 + k/2 + 1} = 2^{(k+1)/2 + k/2 + 1} = 2^{(k+1)/2 + k/2 + 1} = 2^{(k+1)/2 + k/2 + 1} = 2^{(k+1)/2 + k/2 + 1} = 2^{(k+1)/2 + k/2 + 1} = 2^{(k+1)/2 + k/2 + 1} = 2^{(k+1)/2 + k/2 + 1} = 2^{(k+1)/2 + k/2 + 1} = 2^{(k+1)/2 + k/2 + 1} = 2^{(k+1)/2 + k/2 + 1} = 2^{(k+1)/2 + k/2 + 1} = 2^{(k+1)/2 + k/2 + 1} = 2^{(k+1)/2 + k/2 + 1} = 2^{(k+1)/2 + k/2 + 1} = 2^{(k+1)/2 + k/2 + 1} = 2^{(k+1)/2 + k/2 + 1} = 2^{(k+1)/2 + k/2 + 1} = 2^{(k+1)/2 + k/2 + 1} = 2^{(k+1)/2 + k/2 + 1} = 2^{(k+1)/2 + k/2 + 1} = 2^{(k+1)/2 + k/2 + 1} = 2^{(k+1)/2 + k/2 + 1} = 2^{(k+1)/2 + k/2 + 1} = 2^{(k+1)/2 + k/2 + 1} = 2^{(k+1)/2 + k/2 + 1} = 2^{(k+1)/2 + k/2 + 1} = 2^{(k+1)/2 + k/2 + 1} = 2^{(k+1)/2 + k/2 + 1} = 2^{(k+1)/2 + k/2 + 1} = 2^{(k+1)/2 + k/2 + 1} = 2^{(k+1)/2 + k/2 + 1} = 2^{(k+1)/2 + k/2 + 1} = 2^{(k+1)/2 + k/2 + 1} = 2^{(k+1)/2 + k/2 + 1} = 2^{(k+1)/2 + k/2 + 1} = 2^{(k+1)/2 + k/2 + 1} = 2^{(k+1)/2 + k/2 + 1} = 2^{(k+1)/2 + k/2 + 1} = 2^{(k+1)/2 + k/2 + 1} = 2^{(k+1)/2 + k/2 + 1} = 2^{(k+1)/2 + k/2 + 1} = 2^{(k+1)/2 + k/2 + 1} = 2^{(k+1)/2 + k/2 + 1} = 2^{(k+1)/2 + k/2 + 1} = 2^{(k+1)/2 + k/2 + 1} = 2^{(k+1)/2 + k/2 + 1} = 2^{(k+1)/2 + k/2 + 1} = 2^{(k+1)/2 + k/2 + 1} = 2^{(k+1)/2 + k/2 + 1} = 2^{(k+1)/2 + k/2 + 1} = 2^{(k+1)/2 + k/2 + 1} = 2^{(k+1)/2 + k/2 + 1} = 2^{(k+1)/2 + k/2 + 1} = 2^{(k+1)/2 + k/2 + 1} = 2^{(k+1)/2 + k/2 + 1} = 2^{(k+1)/2 + k/2 + 1} = 2^{(k+1)/2 + k/2 + 1} = 2^{(k+1)/2 + k/2 + 1} = 2^{(k+1)/2 + k/2 + 1} = 2^{(k+1)/2 + k/2 + 1} = 2^{(k+1)/2 + k/2 + 1} = 2^{(k+1)/2 + k/2 + 1} = 2^{(k+1)/2 + k/2 + 1} = 2^{(k+1)/2 + k/2 + 1} = 2^{(k+1)/2 + k/2 + 1} = 2^{(k+1)/2 + k/2 + 1} = 2^{(k+1)/2 + k/2 + 1} = 2^{(k+1)/2 + k/2 + 1} = 2^{(k+1)/2 + k/2 + 1} = 2^{(k+1)/2 + k/2 + 1} = 2^{(k+1)/2 + k/2 + 1} = 2^{(k+1)/2 + k/2 + 1} = 2^{(k+1)/2 + k/2 + 1} = 2^{(k+1)/2 + k/2 + 1} = 2^{(k+1)/2 + k/2 + 1} = 2^{(k+1)/2 + k/2 + 1} = 2^{(k+1)/2 + k/2 + 1} = 2^{(k+1)/2 + k/2 + 1} = 2^{(k+1)/2 + k/2 + 1} = 2^{(k+1)/2 + k/2 + 1} = 2^{(k+1)/2 + k/2 + 1} = 2^{(k+1)/2 + k/2 + 1} = 2^{(k+1)/2 + k/2 + 1} = 2^{(k+1)/2 + k/2 + 1} = 2^{(k+1)/2 + k/2 + 1} = 2^{(k+1)/2 + k/2 + 1} = 2^{(k+1)/2 + k/2 + 1} = 2^{(k+1)/2 + k/2 + 1} = 2^{(k+1)/2 + k/2 + 1} = 2^{(k+1)/2 + k/2 + 1} = 2^{(k+1)/2 + k/2 + 1} = 2^{(k+1)/2 + k/2 + 1} = 2^{(k+1)/2 + k/2 + 1} = 2^{(k+1)/2 + k/2 + 1} = 2^{(k+1)/2 + k/2 + 1} = 2^{(k+1)/2 + k/2 + 1} = 2^{(k+1)/2 + k/2 + 1} = 2^{(k+1)/2 + k/2 + 1} = 2^{(k+1)/2 + k/2 + 1} = 2^{(k+1)/2 + k/2 + 1} = 2^{(k+1)/2 + k/2 + 1} = 2^{(k+1)/2 + k/2 + 1} = 2^{(k+1)/2 + k/2 + 1} = 2^{(k+1)/2 + k/2 + 1} = 2^{(k+1)/2 + k/2 + 1} = 2^{(k+1)/2 + k/2 + 1} = 2^{(k+1)/2 + k/2 + 1} = 2^{(k+1)/2 + k/2 + 1} = 2^{(k+1)/2 + k/2 + 1} = 2^{(k+1)/2 + k/2 + 1} = 2^{(k+1)/2 + k/2 + 1} = 2^{(k+1)/2 + k/2 + 1} = 2^{(k+1)/2 + k/2 + 1} = 2^{(k+1)/2 + k/2 + 1} = 2^{(k+1)/2 + k/2 + 1} = 2^{(k+1)/2 + k/2 + 1} = 2^{(k+1)/2 + k/2 + 1} = 2^{(k+1)/2 + k/2 + 1} = 2^{(k+1)/2 + k/2 + 1} = 2^{(k+1)/2 + k/2 + 1} = 2^{(k+1)/2 + k/2 + 1} = 2^{(k+1)/2 + k/2 + 1} = 2^{(k+1)/2 + k/2 + 1} = 2^{(k+1)/2 + k/2 + 1} = 2^{(k+1)/2 + k/2 + 1} = 2^{(k+1)/2 + k/2 + 1} = 2^{(k+1)/2 + k/2 + 1} = 2^{(k+1)/2 + k/2 + 1} = 2^{(k+1)/2 + k/2 + 1} = 2^{(k+1)/2 + k/2 + 1} = 2^{(k+1)/2 + k/2 + 1} = 2^{(k+1)/2 + k/2 + 1} = 2^{(k+1)/2 + k/2 + 1} = 2^{(k+1)/2 + k/2 + 1} = 2^{(k+1)/2 + k/2 + 1} = 2^{(k+1)/2 + k/2 + 1} = 2^{(k+1)/2 + k/2 + 1} = 2^{(k+1)/2 + k/2 + 1} = 2^{(k+1)/2 + k/2 + 1} = 2^{(k+1)/2 + k/2 + 1} = 2^{(k+1)/2 + k/2 + 1} = 2^{(k+1)/2 + k/2 + 1} = 2^{(k+1)/2 + k/2 + 1} = 2^{(k+1)/2 + k/2 + 1} = 2^{(k+1)/2 + k/2 + 1} = 2^{(k+1)/2 + k/2 + 1} = 2^{(k+1)/2 + k/2 + 1} = 2^{(k+1)/2 + k/2 + 1} = 2^{(k+1)/2 + k/2 + 1} = 2^{(k+1)/2 + k/2 + 1} = 2^{(k+1)/2 + k/2 + 1} = 2^{(k+1)/2 + k/2 + 1} = 2^{(k+1)/2 + k/2 + 1} = 2^{(k+1)/2 + k/2 + 1} = 2^{(k+1)/2 + k/2 + 1} = 2^{(k+1)/2 + k/2 + 1} = 2^{(k+1)/2 + k/2 + 1} = 2^{(k+1)/2 + k/2 + 1} = 2^{(k+1)/2 + k/2 + 1} = 2^{(k+1)/2 + k/2 + 1} = 2^{(k+1)/2 + k/2 + 1} = 2^{(k+1)/2 + k/2 + 1} = 2^{(k+1)/2 + k/2 + 1} = 2^{(k+1)/2 + k/2 + 1} = 2^{(k+1)/2 + k/2 + 1} = 2^{(k+1)/2 + k/2 + 1} = 2^{(k+1)/2 + k/2 + 1} = 2^{(k+1)/2 + k/2 + 1} = 2^{(k+1)/2 + k/2 + 1} = 2^{(k+1)/2 + k/2 + 1} = 2^{(k+1)/2 + k/2 + 1} = 2^{(k+1)/2 + k/2 + 1} = 2^{(k+1)/2 + k/2 + 1} = 2^{(k+1)/2 + k/2 + 1} = 2^{(k+1)/2 + k/2 + 1} = 2^{(k+1)/2 + k/2 + 1} = 2^{(k+1)/2 + k/2 + 1} = 2^{(k+1)/2 + k/2 + 1} = 2^{(k+1)/2 + k/2 + 1} = 2^{(k+1)/2 + k/2 + 1} = 2^{(k+1)/2 + k/2 + 1} = 2^{(k+1)/2 + k/2 + 1} = 2^{(k+1)/2 + k/2 + 1} = 2^{(k+1)/2 + k/2 + 1} = 2^{(k+1)/2 + k/2 + 1} = 2^{(k+1)/2 + k/2 + 1} = 2^{(k+1)/2 + k/2 + 1} = 2^{(k+1)/2 + k/2 + 1} = 2^{(k+1)/2 + k/2 + 1} = 2^{(k+1)/2 + k/2 + 1} = 2^{(k+1)/2 + k/2 + 1} = 2^{(k+1)/2 + k/2 + 1} = 2^{(k+1)/2 + k/2 + 1} = 2^{(k+1)/2 + k/2 + 1} = 2^{(k+1)/2 + k/2 + 1} = 2^{(k+1)/2 + k/2 + 1} = 2^{(k+1)/2 + k/2 + 1} = 2^{(k+1)/2 + k/2 + 1} = 2^{(k+1)/2 + k/2 + 1} = 2^{(k+1)/2 + k/2 + 1} = 2^{(k+1)/2 + k/2 + 1} = 2^{(k+1)/2 + k/2 + 1} = 2^{(k+1)/2 + k/2 + 1} = 2^{(k+1)/2 + k/2 + 1} = 2^{(k+1)/2 + k/2 + 1} = 2^{(k+1)/2 + k/2 + 1} = 2^{(k+1)/2 + k/2 + 1} = 2^{(k+1)/2 + k/2 + 1} = 2^{(k+1)/2 + k/2 + 1} = 2^{(k+1)/2 + k/2 + 1} = 2^{(k+1)/2 + k/2 + 1} = 2^{(k+1)/2 + k/2 + 1} = 2^{(k+1)/2 + k/2 + 1} = 2^{(k+1)/2 + k/2 + 1} = 2^{(k+1)/2 + k/2 + 1} = 2^{(k+1)/2 + k/2 + 1} = 2^{(k+1)/2 + k/2 + 1} = 2^{(k+1)/2 + k/2 + 1} = 2^{(k+1)/2 + k/2 + 1} = 2^{(k+1)/2 + k/2 + 1} = 2^{(k+1)/2 + k/2 + 1} = 2^{(k+1)/2 + k/2 + 1} = 2^{(k+1)/2 + k/2 + 1} = 2^{(k+1)/2 + k/2 + 1} = 2^{(k+1)/2 + k/2 + 1} = 2^{(k+1)/2 + k/2 + 1} = 2^{(k+1)/2 + k/2 + 1} = 2^{(k+1)/2 + k/2 + 1} = 2^{(k+1)/2 + k/2 + 1} = 2^{(k+1)/2 + k/2 + 1} = 2^{(k+1)/2 + k/2 + 1} = 2^{(k+1)/2 + k/2 + 1} = 2^{(k+1)/2 + k/2 + 1} = 2^{(k+1)/2 + k/2 + 1} = 2^{(k+1)/2 + k/2 + 1} = 2^{(k+1)/2 + k/2 + 1} = 2^{(k+1)/2 + k/2 + 1} = 2^{(k+1)/2 + k/2 + 1} = 2^{(k+1)/2 + k/2 + 1} = 2^{(k+1)/2 + k/2 + 1} = 2^{(k+1)/2 + k/2 + 1} = 2^{(k+1)/2 + k/2 + 1} = 2^{(k+1)/2 + k/2 + 1} = 2^{(k+1)/2 + k/2 + 1} = 2^{(k+1)/2 + k/2 + 1} = 2^{(k+1)/2 + k/2 + 1} = 2^{(k+1)/2 + k/2 + 1} = 2^{(k+1)/2 + k/2 + 1} = 2^{(k+1)/2 + k/2 + 1} = 2^{(k+1)/2 + k/2 + 1} = 2^{(k+1)/2 + k/2 + 1} = 2^{(k+1)/2 + k/2 + 1} = 2^{(k+1)/2 + k/2 + 1} = 2^{(k+1)/2 + k/2 + 1} = 2^{(k+1)/2 + k/2 + 1} = 2^{(k+1)/2 + k/2 + 1} = 2^{(k+1)/2 + k/2 + 1} = 2^{(k+1)/2 + k/2 + 1} = 2^{(k+1)/2 + k/2 + 1} = 2^{(k+1)/2 + k/2 + 1} = 2^{(k+1)/2 + k/2 + 1} = 2^{(k+1)/2 + k/2 + 1} = 2^{(k+1)/2 + k/2 + 1} = 2^{(k+1)/2 + k/2 + 1} = 2^{(k+1)/2 + k/2 + 1} = 2^{(k+1)/2 + k/2 + 1} = 2^{(k+1)/2 + k/2 + 1} = 2^{(k+1)/2 + k/2 + 1} = 2^{(k+1)/2 + k/2 + 1} = 2^{(k+1)/2 + k/2 + 1} = 2^{(k+1)/2 + k/2 + 1} = 2^{(k+1)/2 + k/2 + 1} = 2^{(k+1)/2 + k/2 + 1} = 2^{(k+1)/2 + k/2 + 1} = 2^{(k+1)/2 + k/2 + 1} = 2^{(k+1)/2 + k/2 + 1} = 2^{(k+1)/2 + k/2 + 1} = 2^{(k+1)/2 + k/2 + 1} = 2^{(k+1)/2 + k/2 + 1} = 2^{(k+1)/2 + k/2 + 1} = 2^{(k+1)/2 + k/2 + 1} = 2^{(k+1)/2 + k/2 + 1} = 2^{(k+1)/2 + k/2 + 1} = 2^{(k+1)/2 + k/2 + 1} = 2^{(k+1)/2 + k/2 + 1} = 2^{(k+1)/2 + k/2 + 1} = 2^{(k+1)/2 + k/2 + 1} = 2^{(k+1)/2 + k/2 + 1} = 2^{(k+1)/2 + k/2 + 1} = 2^{(k+1)/2 + k/