
To solve the definite integral \(\int_0^1 \frac{x-1}{(x+1)\ln x} \, dx\), we proceed as follows:


### Step 1: Recognize the Integral Form
The integrand involves \(\frac{x-1}{\ln x}\), which can be expressed as an integral using the identity:
\[
\frac{x - 1}{\ln x} = \int_0^1 x^t \, dt
\]
This identity holds because \(\int_0^1 x^t \, dt = \left. \frac{x^t}{\ln x} \right|_0^1 = \frac{x - 1}{\ln x}\).


### Step 2: Rewrite the Integral
Substituting this identity into the original integral, we get:
\[
\int_0^1 \frac{x-1}{(x+1)\ln x} \, dx = \int_0^1 \int_0^1 \frac{x^t}{x+1} \, dt \, dx
\]
By Fubini's theorem, we switch the order of integration:
\[
\int_0^1 \int_0^1 \frac{x^t}{x+1} \, dx \, dt
\]


### Step 3: Evaluate the Inner Integral
We focus on the inner integral \(\int_0^1 \frac{x^t}{x+1} \, dx\). Using the power series expansion of \(\frac{1}{x+1}\) for \(|x| < 1\):
\[
\frac{1}{x+1} = \sum_{n=0}^\infty (-1)^n x^n
\]
Substituting this into the inner integral and interchanging summation and integration (justified by uniform convergence), we get:
\[
\int_0^1 \frac{x^t}{x+1} \, dx = \sum_{n=0}^\infty (-1)^n \int_0^1 x^{t+n} \, dx = \sum_{n=0}^\infty \frac{(-1)^n}{t + n + 1}
\]


### Step 4: Relate to the Digamma Function
The sum \(\sum_{n=0}^\infty \frac{(-1)^n}{t + n + 1}\) can be expressed using the digamma function \(\psi(z)\). Using the identity for alternating harmonic series:
\[
\sum_{n=0}^\infty \frac{(-1)^n}{n + a} = \frac{1}{2} \left( \psi\left( \frac{a+1}{2} \right) - \psi\left( \frac{a}{2} \right) \right)
\]
Here, \(a = t + 1\), so the inner integral becomes:
\[
\int_0^1 \frac{x^t}{x+1} \, dx = \frac{1}{2} \left( \psi\left( \frac{t+2}{2} \right) - \psi\left( \frac{t+1}{2} \right) \right)
\]


### Step 5: Integrate Over \(t\)
Substituting back, the original integral becomes:
\[
\int_0^1 \frac{1}{2} \left( \psi\left( \frac{t+2}{2} \right) - \psi\left( \frac{t+1}{2} \right) \right) dt
\]
Using the substitution \(u = \frac{t+1}{2}\) (so \(t = 2u - 1\) and \(dt = 2du\)), the limits change from \(t=0\) to \(u=1/2\) and \(t=1\) to \(u=1\). The integral simplifies to:
\[
\int_{1/2}^1 \left( \psi\left( u + \frac{1}{2} \right) - \psi(u) \right) du
\]


### Step 6: Integrate the Digamma Function
The integral of the digamma function \(\psi(z)\) is \(\ln \Gamma(z)\), where \(\Gamma(z)\) is the gamma function. Thus:
\[
\int \psi(z) \, dz = \ln \Gamma(z) + C
\]
Evaluating the integral over \([1/2, 1]\):
\[
\left[ \ln \Gamma\left( u + \frac{1}{2} \right) - \ln \Gamma(u) \right]_{1/2}^1
\]


### Step 7: Simplify Using Gamma Function Properties
Using \(\Gamma(1) = 1\), \(\Gamma\left( \frac{1}{2} \right) = \sqrt{\pi}\), and \(\Gamma\left( \frac{3}{2} \right) = \frac{\sqrt{\pi}}{2}\), we find:
\[
\left( \ln \Gamma\left( \frac{3}{2} \right) - \ln \Gamma(1) \right) - \left( \ln \Gamma(1) - \ln \Gamma\left( \frac{1}{2} \right) \right) = \left( \ln \frac{\sqrt{\pi}}{2} - 0 \right) - \left( 0 - \ln \sqrt{\pi} \right)
\]
Simplifying further:
\[
\ln \frac{\sqrt{\pi}}{2} + \ln \sqrt{\pi} = \ln \left( \frac{\sqrt{\pi}}{2} \cdot \sqrt{\pi} \right) = \ln \frac{\pi}{2}
\]


### Exact and Numerical Results
The exact value of the integral is \(\ln \frac{\pi}{2}\). Numerically, \(\ln \frac{\pi}{2} \approx 0.4515827053\).


{"answer": "\(\ln \frac{\pi}{2}\)", "numerical_answer": "0.4515827053"}