We wish to evaluate

  I = ∫₀² x^(–1/2) (2 – x)^(–1/2) (1 + 0.5x)^(–1–1) T₂(√(1+0.5x)) dx.

Step 1. Write the integrand in a simpler form.

a) Note that
  (1 + 0.5x)^(–1–1) = (1 + 0.5x)^(–2).

b) The Chebyshev polynomial T₂(z) (of the first kind) satisfies
  T₂(z) = 2z² – 1.
Thus, with z = √(1 + 0.5x) we have
  T₂(√(1+0.5x)) = 2(1+0.5x) – 1 = (2 + x – 1) = x + 1.

So the integrand becomes
  x^(–1/2) (2–x)^(–1/2) (1+0.5x)^(–2) (x+1).

That is, our integral is

  I = ∫₀² (x+1) / [√x √(2–x) · (1+0.5x)²] dx.

Step 2. Make the substitution x = 2 sin²θ.
  Then when x = 0  ⇒ θ = 0,
      x = 2  ⇒ sin²θ = 1 ⇒ θ = π/2.
Differentiate:
  dx = 4 sinθ cosθ dθ.
Also, note that
  √x = √(2 sin²θ) = √2 · sinθ,
  √(2–x) = √(2 – 2 sin²θ) = √(2 cos²θ) = √2 · cosθ.
Thus,
  √x √(2–x) = (√2 sinθ)(√2 cosθ) = 2 sinθ cosθ.

Now, express the remaining factors:
  1 + 0.5x = 1 + 0.5·(2 sin²θ) = 1 + sin²θ,
  x + 1 = 2 sin²θ + 1 = 1 + 2 sin²θ.

Substitute into I:
  I = ∫₀^(π/2) [ (1+2 sin²θ) / ((1+ sin²θ)²) ] · [dx/(2 sinθ cosθ) ].
But dx = 4 sinθ cosθ dθ so
  dx/(2 sinθ cosθ) = (4 sinθ cosθ dθ)/(2 sinθ cosθ) = 2 dθ.

Thus, the integral becomes
  I = 2 ∫₀^(π/2) (1+2 sin²θ)/(1+ sin²θ)² dθ.

Step 3. Split the integrand.
Notice that we can write
  (1+2 sin²θ)/(1+ sin²θ)² = 1/(1+ sin²θ) + sin²θ/(1+ sin²θ)².
Thus, write
  I = 2 [ I₁ + I₂ ],
with
  I₁ = ∫₀^(π/2) dθ/(1+ sin²θ),
  I₂ = ∫₀^(π/2) sin²θ/(1+ sin²θ)² dθ.

Step 4. Evaluate I₁.
There is a standard formula:
  ∫₀^(π/2) dθ/(1 + m sin²θ) = π/(2√(1+m)).
For m = 1 we get
  I₁ = π/(2√2).

Step 5. Evaluate I₂.
A neat observation helps. Write
  sin²θ/(1+ sin²θ)² = 1/(1+ sin²θ) – 1/(1+ sin²θ)².
Thus,
  I₂ = ∫₀^(π/2) [1/(1+ sin²θ) – 1/(1+ sin²θ)²] dθ = I₁ – I₃,
with
  I₃ = ∫₀^(π/2) dθ/(1+ sin²θ)².

A standard formula (which can be obtained by differentiating the formula for I₁ with respect to the parameter m) gives:
  I₃ = ∫₀^(π/2) dθ/(1+ sin²θ)² = (3π)/(8√2).

Thus,
  I₂ = I₁ – I₃ = (π/(2√2)) – (3π/(8√2)) = (4π – 3π)/(8√2) = (π)/(8√2).

Step 6. Combine the pieces.
We had
  I = 2 (I₁ + I₂) = 2 [ (π/(2√2)) + (π/(8√2)) ].
Combine the fractions:
  (π/(2√2)) + (π/(8√2)) = (4π + π)/(8√2) = (5π)/(8√2).
Then,
  I = 2 · (5π/(8√2)) = (5π)/(4√2).

Thus, the exact answer is

  I = (5π)/(4√2).

Step 7. Numerical approximation.
We compute:
  π ≈ 3.141592653589793,
  √2 ≈ 1.414213562373095,
so
  4√2 ≈ 4 × 1.414213562373095 = 5.65685424949238,
and then
  I ≈ (5×3.141592653589793) / 5.65685424949238 ≈ 15.707963267949 / 5.65685424949238 ≈ 2.7768018363.

Thus, the final answers are:

Exact answer: (5π)/(4√2)  and  Numerical value: 2.7768018363.

{"answer": "\\frac{5\\pi}{4\\sqrt{2}}", "numerical_answer": "2.7768018363"}