# Evaluating $\int_{\pi/6}^{\pi/3}\frac{\sin(x)+\cos(x)}{\sqrt{\sin(2x)}}\text{ d}x$

## Step 1: Simplify the integrand
First, recall that $\sin(2x) = 2\sin(x)\cos(x)$. So:

$$\frac{\sin(x)+\cos(x)}{\sqrt{\sin(2x)}} = \frac{\sin(x)+\cos(x)}{\sqrt{2\sin(x)\cos(x)}} = \frac{\sin(x)+\cos(x)}{\sqrt{2}\sqrt{\sin(x)\cos(x)}}$$

## Step 2: Split the integral
$$\int_{\pi/6}^{\pi/3}\frac{\sin(x)+\cos(x)}{\sqrt{\sin(2x)}}\text{ d}x = \int_{\pi/6}^{\pi/3}\frac{\sin(x)}{\sqrt{2}\sqrt{\sin(x)\cos(x)}}\text{ d}x + \int_{\pi/6}^{\pi/3}\frac{\cos(x)}{\sqrt{2}\sqrt{\sin(x)\cos(x)}}\text{ d}x$$

## Step 3: Simplify each part
For the first part:
$$\int_{\pi/6}^{\pi/3}\frac{\sin(x)}{\sqrt{2}\sqrt{\sin(x)\cos(x)}}\text{ d}x = \frac{1}{\sqrt{2}}\int_{\pi/6}^{\pi/3}\frac{\sin(x)}{\sqrt{\sin(x)\cos(x)}}\text{ d}x = \frac{1}{\sqrt{2}}\int_{\pi/6}^{\pi/3}\frac{\sqrt{\sin(x)}}{\sqrt{\cos(x)}}\text{ d}x$$

For the second part:
$$\int_{\pi/6}^{\pi/3}\frac{\cos(x)}{\sqrt{2}\sqrt{\sin(x)\cos(x)}}\text{ d}x = \frac{1}{\sqrt{2}}\int_{\pi/6}^{\pi/3}\frac{\cos(x)}{\sqrt{\sin(x)\cos(x)}}\text{ d}x = \frac{1}{\sqrt{2}}\int_{\pi/6}^{\pi/3}\frac{\sqrt{\cos(x)}}{\sqrt{\sin(x)}}\text{ d}x$$

## Step 4: Make a substitution
Let's try the substitution $u = \tan(x)$. Then:
- $dx = \frac{du}{1+u^2}$
- $\sin(x) = \frac{u}{\sqrt{1+u^2}}$
- $\cos(x) = \frac{1}{\sqrt{1+u^2}}$

When $x = \pi/6$, $u = \tan(\pi/6) = \frac{1}{\sqrt{3}}$
When $x = \pi/3$, $u = \tan(\pi/3) = \sqrt{3}$

For the first integral:
$$\frac{\sqrt{\sin(x)}}{\sqrt{\cos(x)}} = \frac{\sqrt{\frac{u}{\sqrt{1+u^2}}}}{\sqrt{\frac{1}{\sqrt{1+u^2}}}} = \frac{u^{1/2}(1+u^2)^{1/4}}{(1+u^2)^{1/4}} = u^{1/2} = \sqrt{u}$$

For the second integral:
$$\frac{\sqrt{\cos(x)}}{\sqrt{\sin(x)}} = \frac{\sqrt{\frac{1}{\sqrt{1+u^2}}}}{\sqrt{\frac{u}{\sqrt{1+u^2}}}} = \frac{(1+u^2)^{1/4}}{u^{1/2}(1+u^2)^{1/4}} = \frac{1}{\sqrt{u}} = u^{-1/2}$$

## Step 5: Rewrite the integrals
The first integral becomes:
$$\frac{1}{\sqrt{2}}\int_{\frac{1}{\sqrt{3}}}^{\sqrt{3}} \sqrt{u} \cdot \frac{du}{1+u^2} = \frac{1}{\sqrt{2}}\int_{\frac{1}{\sqrt{3}}}^{\sqrt{3}} \frac{u^{1/2}}{1+u^2} du$$

The second integral becomes:
$$\frac{1}{\sqrt{2}}\int_{\frac{1}{\sqrt{3}}}^{\sqrt{3}} \frac{1}{\sqrt{u}} \cdot \frac{du}{1+u^2} = \frac{1}{\sqrt{2}}\int_{\frac{1}{\sqrt{3}}}^{\sqrt{3}} \frac{u^{-1/2}}{1+u^2} du$$

## Step 6: Solve the integrals
For the first integral $\int \frac{u^{1/2}}{1+u^2} du$, I'll use the substitution $v = u^2$:
- $u = \sqrt{v}$
- $du = \frac{dv}{2\sqrt{v}}$

This gives:
$$\int \frac{u^{1/2}}{1+u^2} du = \int \frac{\sqrt{\sqrt{v}}}{1+v} \cdot \frac{dv}{2\sqrt{v}} = \frac{1}{2}\int \frac{v^{1/4}}{1+v} \cdot \frac{dv}{v^{1/2}} = \frac{1}{2}\int \frac{v^{-1/4}}{1+v} dv$$

This is a complex integral. Let's try a different approach.

Let's go back to our original integral and try a different substitution. Let $u = \sqrt{\sin(2x)}$, then $\sin(2x) = u^2$. 

We also know that $\sin(x)+\cos(x) = \sqrt{2}\sin(x+\pi/4)$

So our integral becomes:
$$\int_{\pi/6}^{\pi/3}\frac{\sin(x)+\cos(x)}{\sqrt{\sin(2x)}}\text{ d}x = \int_{\pi/6}^{\pi/3}\frac{\sqrt{2}\sin(x+\pi/4)}{u}\text{ d}x$$

Actually, let's go back to the original form and use properties of trigonometric functions:

$$\int_{\pi/6}^{\pi/3}\frac{\sin(x)+\cos(x)}{\sqrt{\sin(2x)}}\text{ d}x$$

Using the identity $\sin(x)+\cos(x) = \sqrt{2}\sin(x+\pi/4)$:

$$\int_{\pi/6}^{\pi/3}\frac{\sqrt{2}\sin(x+\pi/4)}{\sqrt{\sin(2x)}}\text{ d}x = \sqrt{2}\int_{\pi/6}^{\pi/3}\frac{\sin(x+\pi/4)}{\sqrt{\sin(2x)}}\text{ d}x$$

## Let's try a different approach
From $\sin(2x) = 2\sin(x)\cos(x)$, we have $\sqrt{\sin(2x)} = \sqrt{2\sin(x)\cos(x)}$

Our integral becomes:
$$\int_{\pi/6}^{\pi/3}\frac{\sin(x)+\cos(x)}{\sqrt{2\sin(x)\cos(x)}}\text{ d}x = \frac{1}{\sqrt{2}}\int_{\pi/6}^{\pi/3}\frac{\sin(x)+\cos(x)}{\sqrt{\sin(x)\cos(x)}}\text{ d}x$$

Splitting this:
$$\frac{1}{\sqrt{2}}\left[\int_{\pi/6}^{\pi/3}\frac{\sin(x)}{\sqrt{\sin(x)\cos(x)}}\text{ d}x + \int_{\pi/6}^{\pi/3}\frac{\cos(x)}{\sqrt{\sin(x)\cos(x)}}\text{ d}x\right]$$

For the first part: $\frac{\sin(x)}{\sqrt{\sin(x)\cos(x)}} = \frac{\sqrt{\sin(x)}}{\sqrt{\cos(x)}}$
For the second part: $\frac{\cos(x)}{\sqrt{\sin(x)\cos(x)}} = \frac{\sqrt{\cos(x)}}{\sqrt{\sin(x)}}$

Let's substitute $u = \sin(x)$ for the first integral:
- $du = \cos(x)dx$
- When $x = \pi/6$, $u = \sin(\pi/6) = 1/2$
- When $x = \pi/3$, $u = \sin(\pi/3) = \sqrt{3}/2$

For the first integral:
$$\int_{\pi/6}^{\pi/3}\frac{\sqrt{\sin(x)}}{\sqrt{\cos(x)}}\text{ d}x = \int_{1/2}^{\sqrt{3}/2}\frac{\sqrt{u}}{\sqrt{1-u^2}}\cdot\frac{du}{\cos(x)} = \int_{1/2}^{\sqrt{3}/2}\frac{\sqrt{u}}{\sqrt{1-u^2}}\cdot\frac{du}{\sqrt{1-u^2}} = \int_{1/2}^{\sqrt{3}/2}\frac{\sqrt{u}}{1-u^2}du$$

Let's use $v = \cos(x)$ for the second integral:
- $dv = -\sin(x)dx$
- When $x = \pi/6$, $v = \cos(\pi/6) = \sqrt{3}/2$
- When $x = \pi/3$, $v = \cos(\pi/3) = 1/2$

For the second integral:
$$\int_{\pi/6}^{\pi/3}\frac{\sqrt{\cos(x)}}{\sqrt{\sin(x)}}\text{ d}x = \int_{\sqrt{3}/2}^{1/2}\frac{\sqrt{v}}{\sqrt{1-v^2}}\cdot\frac{-dv}{\sin(x)} = -\int_{\sqrt{3}/2}^{1/2}\frac{\sqrt{v}}{\sqrt{1-v^2}}\cdot\frac{dv}{\sqrt{1-v^2}} = -\int_{\sqrt{3}/2}^{1/2}\frac{\sqrt{v}}{1-v^2}dv$$

Reversing the limits:
$$-\int_{\sqrt{3}/2}^{1/2}\frac{\sqrt{v}}{1-v^2}dv = \int_{1/2}^{\sqrt{3}/2}\frac{\sqrt{v}}{1-v^2}dv$$

So both integrals are identical! This gives us:
$$\frac{1}{\sqrt{2}}\left[2\int_{1/2}^{\sqrt{3}/2}\frac{\sqrt{u}}{1-u^2}du\right] = \frac{2}{\sqrt{2}}\int_{1/2}^{\sqrt{3}/2}\frac{\sqrt{u}}{1-u^2}du = \sqrt{2}\int_{1/2}^{\sqrt{3}/2}\frac{\sqrt{u}}{1-u^2}du$$

## Final solution
Using the substitution $w = u^2$:
- $u = \sqrt{w}$
- $du