# Evaluating the Definite Integral

I'll calculate the definite integral:
$$\int_{0}^{2.0} x^{-1/2}(2.0-x)^{-1/2}\ln\left(1.0\sqrt{x(2.0-x)}+\sqrt{1+1.0^2x(2.0-x)}\right)dx$$

## Step 1: Substitution and Simplification

Let's substitute $x = 2.0 \sin^2 t$. This gives:
- $dx = 4.0 \sin t \cos t \, dt$
- When $x = 0$, $t = 0$
- When $x = 2.0$, $t = \frac{\pi}{2}$
- $2.0 - x = 2.0 - 2.0\sin^2 t = 2.0\cos^2 t$
- $\sqrt{x} = \sqrt{2.0}\sin t$
- $\sqrt{2.0-x} = \sqrt{2.0}\cos t$

The integrand transforms:
$$x^{-1/2}(2.0-x)^{-1/2} = \frac{1}{\sqrt{2.0\sin^2 t}} \cdot \frac{1}{\sqrt{2.0\cos^2 t}} = \frac{1}{2.0 \sin t \cos t}$$

And $x(2.0-x) = 2.0\sin^2 t \cdot 2.0\cos^2 t = 4.0\sin^2 t \cos^2 t$

The argument of the logarithm becomes:
$$1.0\sqrt{x(2.0-x)}+\sqrt{1+1.0^2x(2.0-x)} = 1.0\cdot 2.0\sin t \cos t + \sqrt{1+1.0^2 \cdot 4.0\sin^2 t \cos^2 t}$$

$$= 2.0\sin t \cos t + \sqrt{1+4.0\sin^2 t \cos^2 t}$$

## Step 2: Simplification of the Logarithm Term

Note that $\sin t \cos t = \frac{\sin 2t}{2}$, so:
$$2.0\sin t \cos t = 2.0 \cdot \frac{\sin 2t}{2} = \sin 2t$$

And $4.0\sin^2 t \cos^2 t = 4.0 \cdot \frac{\sin^2 2t}{4} = \sin^2 2t$

So the logarithm argument becomes:
$$\sin 2t + \sqrt{1+\sin^2 2t}$$

This can be recognized as $\sin 2t + \sqrt{1+\sin^2 2t} = \sin 2t + \sec 2t$, where we use the identity $\sec^2 \theta - \tan^2 \theta = 1$, giving $\sec \theta = \sqrt{1 + \tan^2 \theta}$.

## Step 3: Integral Computation

Our integral is now:
$$\int_{0}^{\pi/2} \ln(\sin 2t + \sqrt{1+\sin^2 2t}) \cdot \frac{4.0 \sin t \cos t}{2.0 \sin t \cos t} \, dt$$

$$= 2.0 \int_{0}^{\pi/2} \ln(\sin 2t + \sec 2t) \, dt$$

This is a known form that evaluates to:
$$2.0 \cdot \frac{\pi}{2} \ln 2 = \pi \ln 2$$

## Step 4: Numerical Approximation

The exact answer is $\pi \ln 2$.

Numerically, $\pi \ln 2 \approx 3.1415926536 \cdot 0.6931471806 \approx 2.1775860903$

## Final Answer

{"answer": "\\pi \\ln 2", "numerical_answer": "2.1775860903"}