We wish to evaluate
  I = ∫₀∞ [x²/(eˣ – 1)]·[2³ sinh(0.5x) – sinh(0.25x)] dx.
In other words,
  I = ∫₀∞ (x²/(eˣ – 1))·[8 sinh(x/2) – sinh(x/4)] dx.

It turns out that a convenient way to proceed is to expand 1/(eˣ – 1) in a sum and then use the standard Laplace transform for x²·e^(–αx).

Step 1. Write the series expansion

Recall that for x > 0,
  1/(eˣ – 1) = ∑ₙ₌₁∞ e^(–n x).
Hence, we may write
  I = ∑ₙ₌₁∞ ∫₀∞ x² e^(–n x) [8 sinh(x/2) – sinh(x/4)] dx.
Interchange summation and integration (which is justified by absolute convergence).

Step 2. Write the hyperbolic sine functions in exponential form

For any real a we have
  sinh(a x) = (e^(a x) – e^(–a x))/2.
Thus, the integrals in I split into sums of integrals of the form
  ∫₀∞ x² e^(–λx) dx,
with various shift parameters λ.

We separate I into two parts:
  I = 8 I₁ – I₂,
with
  I₁ = ∑ₙ₌₁∞ ∫₀∞ x² e^(–n x) sinh(x/2) dx,
  I₂ = ∑ₙ₌₁∞ ∫₀∞ x² e^(–n x) sinh(x/4) dx.

Step 3. Evaluate I₁

Write
  sinh(x/2) = ½ (e^(x/2) – e^(–x/2)).
Thus,
  I₁ = ∑ₙ₌₁∞ ½ [∫₀∞ x² e^(–(n – ½)x) dx – ∫₀∞ x² e^(–(n + ½)x) dx].
We use the standard formula
  ∫₀∞ x² e^(–λx) dx = 2!/λ³ = 2/λ³.
Thus,
  I₁ = ∑ₙ₌₁∞ ½ [2/(n – ½)³ – 2/(n + ½)³] = ∑ₙ₌₁∞ [1/(n – ½)³ – 1/(n + ½)³].

This sum can be written in terms of the Hurwitz zeta function ζ(s, q) which is defined by
  ζ(s, q) = ∑ₙ₌₀∞ 1/(n + q)^s.
Notice that
  ∑ₙ₌₁∞ 1/(n – ½)³ = ∑ₙ₌₀∞ 1/(n + ½)³ = ζ(3, ½)
and
  ∑ₙ₌₁∞ 1/(n + ½)³ = ζ(3, 3/2).
Thus, we may write
  I₁ = ζ(3, ½) – ζ(3, 3/2).

Now use the identity
  ζ(s, q+1) = ζ(s, q) – 1/qˢ.
For s = 3 and q = ½, we have
  ζ(3, 3/2) = ζ(3, ½) – (1/(½)³) = ζ(3, ½) – 8.
Thus,
  I₁ = ζ(3, ½) – [ζ(3, ½) – 8] = 8.

Step 4. Evaluate I₂

Similarly, using
  sinh(x/4) = ½ (e^(x/4) – e^(–x/4)),
we have
  I₂ = ∑ₙ₌₁∞ ½ [∫₀∞ x² e^(–(n – ¼)x) dx – ∫₀∞ x² e^(–(n + ¼)x) dx]
     = ∑ₙ₌₁∞ [1/(n – ¼)³ – 1/(n + ¼)³].
Express the sums in terms of the Hurwitz zeta function:
  ∑ₙ₌₁∞ 1/(n – ¼)³ = ζ(3, ¾)    (since n – ¼ = (n–1)+¾)
and
  ∑ₙ₌₁∞ 1/(n + ¼)³ = ζ(3, 5/4).
Thus,
  I₂ = ζ(3, ¾) – ζ(3, 5/4).

Now use the identity with s=3 and q = ¾:
  ζ(3, 5/4) = ζ(3, ¾) – (1/(¾)³) = ζ(3, ¾) – (64/27).
Hence,
  I₂ = ζ(3, ¾) – [ζ(3, ¾) – 64/27] = 64/27.

Step 5. Combine the results

We found:
  I₁ = 8  and  I₂ = 64/27.
Thus, the overall integral is
  I = 8 I₁ – I₂ = 8·8 – 64/27 = 64 – 64/27.
Write 64 as (64*27)/27:
  I = (64·27 – 64)/27 = (64(27 – 1))/27 = (64·26)/27 = 1664/27.

Step 6. Numerical approximation

Compute 1664/27:
  1664 ÷ 27 ≈ 61.6296296296…
Rounded to 10 decimal places, this is approximately 61.6296296296.

Final Answer in JSON:
{"answer": "\\frac{1664}{27}", "numerical_answer": "61.6296296296"}