We start with

  I = ∫₀² H₃(√(x(2 – x))) dx

where the physicists’ Hermite polynomial of degree 3 is given by

  H₃(t) = 8t³ – 12t.

Thus the integrand becomes

  H₃(√(x(2 – x))) = 8 (x(2 – x))^(3/2) – 12 (x(2 – x))^(1/2),

and so

  I = 8 ∫₀² (x(2 – x))^(3/2) dx – 12 ∫₀² (x(2 – x))^(1/2) dx.

A useful substitution is to let

  x = 1 + cos θ.
Then
  2 – x = 1 – cos θ, and x(2 – x) = (1 + cos θ)(1 – cos θ) = 1 – cos²θ = sin²θ.
Also, dx = – sin θ dθ.

The limits change as follows:
  When x = 0: 0 = 1 + cos θ ⟹ cos θ = –1 ⟹ θ = π.
  When x = 2: 2 = 1 + cos θ ⟹ cos θ = 1 ⟹ θ = 0.

Let’s transform each term.

For the first integral,
  I₁ = ∫₀² (x(2 – x))^(3/2) dx = ∫ₜ₌π⁰ (sin²θ)^(3/2) (– sin θ dθ)
     = ∫ₜ₌π⁰ sin³θ (– sin θ dθ)
     = ∫ₜ₌π⁰ (– sin⁴θ dθ)
Changing the limits,
  I₁ = ∫₀^π sin⁴θ dθ.

For the second integral,
  I₂ = ∫₀² (x(2 – x))^(1/2) dx = ∫ₜ₌π⁰ (sin²θ)^(1/2)(– sin θ dθ)
     = ∫ₜ₌π⁰ sin θ (– sin θ dθ)
     = ∫ₜ₌π⁰ (– sin²θ dθ)
Changing the limits,
  I₂ = ∫₀^π sin²θ dθ.

Thus, the original integral transforms into

  I = 8 I₁ – 12 I₂ = 8 ∫₀^π sin⁴θ dθ – 12 ∫₀^π sin²θ dθ.

We now recall the standard integrals:
  ∫₀^π sin²θ dθ = π/2,
  ∫₀^π sin⁴θ dθ = 3π/8.
(These results can be derived using standard reduction formulas or the Beta function.)

Substituting, we get
  I = 8 × (3π/8) – 12 × (π/2)
     = 3π – 6π
     = –3π.

Thus, the exact answer is –3π.

Numerically, –3π ≈ –3 × 3.1415926536 ≈ –9.4247779608.

{"answer": "-3\\pi", "numerical_answer": "-9.4247779608"}