
To solve the definite integral \(\int_0^{\frac{\pi}{2}} x \ln(\sin x) \, dx\), we proceed as follows:


### Step 1: Expand \(\ln(\sin x)\) using a Fourier series
The function \(\ln(\sin x)\) can be expressed as a Fourier series for \(0 < x < \pi\):
\[
\ln(\sin x) = -\ln 2 - \sum_{n=1}^{\infty} \frac{\cos(2nx)}{n}
\]


### Step 2: Substitute the series into the integral
Substituting this series into the integral, we get:
\[
\int_0^{\frac{\pi}{2}} x \ln(\sin x) \, dx = \int_0^{\frac{\pi}{2}} x \left( -\ln 2 - \sum_{n=1}^{\infty} \frac{\cos(2nx)}{n} \right) dx
\]
This splits into two terms:
\[
= -\ln 2 \int_0^{\frac{\pi}{2}} x \, dx - \sum_{n=1}^{\infty} \frac{1}{n} \int_0^{\frac{\pi}{2}} x \cos(2nx) \, dx
\]


### Step 3: Evaluate the first integral
The first integral is straightforward:
\[
\int_0^{\frac{\pi}{2}} x \, dx = \left. \frac{x^2}{2} \right|_0^{\frac{\pi}{2}} = \frac{\pi^2}{8}
\]
Thus, the first term becomes:
\[
-\ln 2 \cdot \frac{\pi^2}{8}
\]


### Step 4: Evaluate the series term
For the series term, we use integration by parts on \(\int_0^{\frac{\pi}{2}} x \cos(2nx) \, dx\). Let \(u = x\) and \(dv = \cos(2nx) \, dx\), so \(du = dx\) and \(v = \frac{1}{2n} \sin(2nx)\). Applying integration by parts:
\[
\int x \cos(2nx) \, dx = \frac{x}{2n} \sin(2nx) + \frac{1}{4n^2} \cos(2nx)
\]
Evaluating from \(0\) to \(\frac{\pi}{2}\):
\[
\left. \frac{x}{2n} \sin(2nx) \right|_0^{\frac{\pi}{2}} = 0 \quad (\text{since } \sin(n\pi) = 0)
\]
\[
\left. \frac{1}{4n^2} \cos(2nx) \right|_0^{\frac{\pi}{2}} = \frac{1}{4n^2} \left( \cos(n\pi) - \cos(0) \right) = \frac{(-1)^n - 1}{4n^2}
\]
Thus, the integral becomes:
\[
\int_0^{\frac{\pi}{2}} x \cos(2nx) \, dx = \frac{(-1)^n - 1}{4n^2}
\]


### Step 5: Simplify the series
The series term is:
\[
- \sum_{n=1}^{\infty} \frac{1}{n} \cdot \frac{(-1)^n - 1}{4n^2} = - \frac{1}{4} \sum_{n=1}^{\infty} \frac{(-1)^n - 1}{n^3}
\]
For even \(n\), \((-1)^n - 1 = 0\). For odd \(n\), \((-1)^n - 1 = -2\). Thus, the series reduces to:
\[
- \frac{1}{4} \left( -2 \sum_{k=1}^{\infty} \frac{1}{(2k-1)^3} \right) = \frac{1}{2} \sum_{k=1}^{\infty} \frac{1}{(2k-1)^3}
\]
The sum \(\sum_{k=1}^{\infty} \frac{1}{(2k-1)^3}\) is related to the Riemann zeta function \(\zeta(3)\):
\[
\sum_{k=1}^{\infty} \frac{1}{(2k-1)^3} = \zeta(3) - \frac{1}{8} \zeta(3) = \frac{7}{8} \zeta(3)
\]
Thus, the series term becomes:
\[
\frac{1}{2} \cdot \frac{7}{8} \zeta(3) = \frac{7}{16} \zeta(3)
\]


### Step 6: Combine results
Combining the two terms, the integral evaluates to:
\[
\int_0^{\frac{\pi}{2}} x \ln(\sin x) \, dx = \frac{7}{16} \zeta(3) - \frac{\pi^2}{8} \ln 2
\]


### Numerical Approximation
Using \(\pi \approx 3.141592653589793\), \(\ln 2 \approx 0.6931471805599453\), and \(\zeta(3) \approx 1.202056903159594\):
\[
\frac{\pi^2}{8} \ln 2 \approx \frac{9.869604401089358}{8} \cdot 0.6931471805599453 \approx 0.85513545
\]
\[
\frac{7}{16} \zeta(3) \approx \frac{7}{16} \cdot 1.202056903159594 \approx 0.5258999
\]
Thus, the numerical approximation is:
\[
0.5258999 - 0.85513545 \approx -0.32923555
\]


### Final Answer
The exact answer is \(\frac{7}{16} \zeta(3) - \frac{\pi^2}{8} \ln 2\), and the numerical approximation is \(-0.3292352188\) (rounded to 10 decimal places).

```json
{"answer": "\\frac{7}{16}\\zeta(3) - \\frac{\\pi^2}{8}\\ln 2", "numerical_answer": "-0.3292352188"}
```