<think>
Okay, let's tackle this integral step by step. The integral given is from 0 to 1 of (sin(log x) - log x) divided by (log x squared) dx. Hmm, that looks a bit complicated, but maybe substitution can help. 

First, I notice that the integrand has log x in multiple places. Maybe substituting t = log x would simplify things. Let's try that. If t = log x, then dt/dx = 1/x, so dx = x dt. But since t = log x, x is e^t. So dx = e^t dt. 

Now, the limits of integration: when x approaches 0 from the right, log x approaches negative infinity. When x is 1, log x is 0. So the integral becomes from t = -infty to t = 0 of [sin(t) - t]/t² * e^t dt. Wait, let me check that substitution again. The original integrand is [sin(log x) - log x]/(log x)^2 dx. Substituting t = log x, so x = e^t, dx = e^t dt. Then the integrand becomes [sin(t) - t]/t² * e^t dt. So the integral is from t = -infty to t = 0. 

But integrating from -infty to 0 might be tricky. Maybe we can switch the limits to make it from 0 to infty by substituting t = -u. Let me see. Let u = -t, so when t approaches -infty, u approaches infty, and when t=0, u=0. Then dt = -du. So the integral becomes from u=infty to u=0 of [sin(-u) - (-u)]/( (-u)^2 ) * e^{-u} (-du). Let's simplify that. 

sin(-u) is -sin u, and (-u)^2 is u². The numerator becomes (-sin u + u) = (u - sin u). The negative sign from dt = -du flips the limits back to 0 to infty. So the integral becomes ∫₀^∞ [u - sin u]/u² * e^{-u} du. That seems more manageable. 

So now the integral is ∫₀^∞ (u - sin u)/u² * e^{-u} du. Let's split this into two integrals: ∫₀^∞ (u e^{-u})/u² du - ∫₀^∞ (sin u e^{-u})/u² du. Simplifying the first integral: ∫₀^∞ e^{-u}/u du. Wait, but 1/u integrated from 0 to infinity might be problematic. Hmm, maybe integrating by parts would help here. 

Alternatively, let's consider the entire expression (u - sin u)/u². Maybe we can express this as ∫₀^∞ [ (1/u - sin u / u² ) ] e^{-u} du. Hmm, perhaps integrating each term separately. Let's look at the first term: ∫₀^∞ e^{-u}/u du. Wait, that integral is actually divergent because near u=0, 1/u blows up. But the original integral from 0 to 1 in x corresponds to t from -infty to 0, which after substitution becomes u from 0 to infty. But if the integral after substitution has a term, maybe there's cancellation between the two terms. Because the original integrand might have a removable singularity at x=1 (where log x=0). Let me check the original integrand as x approaches 1. 

When x approaches 1, log x approaches 0. Let's expand sin(log x) around log x =0. sin(z) ≈ z - z^3/6 + ... So sin(z) - z ≈ -z^3/6. Then the numerator is -z^3/6, denominator is z², so overall -z/6. As z approaches 0, the integrand approaches 0. So the integrand is actually well-behaved at x=1. Similarly, as x approaches 0, log x approaches -infty. Let's see the behavior there. The integrand is [sin(log x) - log x]/(log x)^2. Let t = log x, so t approaches -infty. Then the integrand becomes [sin t - t]/t². As t approaches -infty, sin t oscillates between -1 and 1, so sin t is negligible compared to -t. So the numerator is approximately -t, denominator t², so overall -1/t. So the integrand behaves like -1/t as t approaches -infty. Then when multiplied by dx = e^t dt, the integrand becomes (-1/t) e^t. As t approaches -infty, e^t approaches 0 exponentially, so the integrand behaves like e^t}/|t|, which tends to 0. So the integral should be convergent. 

But when we split into two integrals, each might be divergent parts, but their combination converges. So maybe we need to handle them together. Alternatively, perhaps integrating by parts. Let's try integrating by parts the original integral. Let me consider the integral after substitution: ∫₀^∞ [u - sin u]/u² e^{-u} du. Let me write this as ∫₀^∞ [ (1/u - sin u / u² ) ] e^{-u} du. Let's split into two integrals: I1 = ∫₀^∞ e^{-u}/u du and I2 = ∫₀^∞ e^{-u} sin u / u² du. But I1 is divergent. However, perhaps the combination I1 - I2 is convergent. 

Alternatively, maybe we can combine the terms. Let's consider integrating [u - sin u]/u² e^{-u} du. Let me write this as ∫ [ (1/u - sin u / u² ) ] e^{-u} du. Let's consider integrating the first term, 1/u e^{-u} du. Let me set v = 1/u, dw = e^{-u} du. Then dv = -1/u² du, w = -e^{-u}. Integration by parts gives v w - ∫ w dv = (1/u)(-e^{-u}) - ∫ (-e^{-u})(-1/u²) du. Which is -e^{-u}/u - ∫ e^{-u}/u² du. Hmm, so that's the first term. Then the original integral is I = ∫ [1/u e^{-u} - sin u / u² e^{-u} ] du. Let me write this as I = ∫1/u e^{-u} du - ∫ sin u / u² e^{-u} du. 

But from the integration by parts above, ∫1/u e^{-u} du = -e^{-u}/u - ∫ e^{-u}/u² du. So substituting back into I: I = [ -e^{-u}/u - ∫ e^{-u}/u² du ] - ∫ sin u / u² e^{-u} du. Then I = -e^{-u}/u | from 0 to ∞ - ∫ e^{-u}/u² du - ∫ sin u / u² e^{-u} du. 

But evaluating the first term at the limits: as u approaches ∞, e^{-u}/u approaches 0. As u approaches 0, e^{-u} ≈1, so -e^{-u}/u approaches -1/0 which is -infinity. Wait, but this seems problematic. But maybe the original approach is not the best. Let's think differently. 

Alternatively, perhaps consider differentiating under the integral sign. Let me define a parameterized integral. Let’s consider F(a) = ∫₀^∞ [u - sin u]/u² e^{-a u} du. Then our integral is F(1). Maybe compute F(a) and then set a=1. 

But how to compute F(a)? Let's split it into two integrals: F(a) = ∫₀^∞ (u e^{-a u})/u² du - ∫₀^∞ (sin u e^{-a u})/u² du = ∫₀^∞ e^{-a u}/u du - ∫₀^∞ sin u e^{-a u}/u² du. But again, the first integral is divergent. Hmm. 

Alternatively, perhaps consider integrating with respect to a. Let me see. Let’s take the Laplace transform approach. The integral involves e^{-a u}, so maybe relate it to Laplace transforms. The Laplace transform of sin u is 1/(s² +1), but here we have sin u / u². Maybe integrating or differentiating known transforms. 

Alternatively, consider integrating the original integral by parts. Let me take the original integral after substitution: ∫₀^∞ [u - sin u]/u² e^{-u} du. Let me write this as ∫₀^∞ [ (1/u - sin u / u² ) ] e^{-u} du. Let’s consider integrating the entire expression by parts. Let’s set v = [u - sin u ]/u², dw = e^{-u} du. Then dv would be [ (1 - cos u)u² - 2u(u - sin u) ] / u^4 du. Hmm, that seems complicated. Maybe not the best approach. 

Wait, perhaps another substitution. Let’s consider t = u, and see if we can express the integral in terms of known functions. Let me recall that ∫ e^{-a u} sin u du is a standard integral. But here we have sin u / u². Maybe integrating by parts. Let’s take the second term: ∫₀^∞ (sin u / u²) e^{-u} du. Let’s set v = sin u / u², dw = e^{-u} du. Then dv = [cos u / u² - 2 sin u / u³] du, and w = -e^{-u}. Integration by parts gives v w | from 0 to ∞ - ∫ w dv. 

Evaluating the boundary term: as u approaches ∞, sin u / u² * e^{-u} approaches 0. As u approaches 0, sin u ≈ u, so sin u / u² ≈ 1/u, multiplied by e^{-u} ≈1, so the term is approximately 1/u, which tends to infinity. But multiplied by w = -e^{-u} which is -1 at u approaches 0. So the boundary term would be [0 - (-1 * 0)]? Wait, maybe not. Let me compute the limit as u approaches 0 of [sin u / u² * (-e^{-u})]. As u approaches 0, sin u ~ u - u^3/6, so sin u / u² ~ 1/u - u/6. Multiply by -e^{-u} ~ -1 + u. So the term is (-1/u + ...) as u approaches 0. But this would go to -infinity. But the original integral is supposed to be convergent. So perhaps integrating by parts here is not helpful. 

Hmm, maybe another approach. Let's consider the integral ∫₀^1 [sin(log x) - log x]/(log x)^2 dx. Let me make substitution t = -log x, so x = e^{-t}, dx = -e^{-t} dt. When x=0, t approaches infinity, x=1, t=0. So the integral becomes ∫_{∞}^0 [sin(-t) - (-t)] / (-t)^2 * (-e^{-t}) dt. Simplify the terms: sin(-t) = -sin t, (-t)^2 = t², and the negative sign from dx flips the limits. So integral becomes ∫₀^∞ [ -sin t + t ] / t² * e^{-t} dt = ∫₀^∞ (t - sin t)/t² e^{-t} dt. Which is the same as before. 

So maybe we can write (t - sin t)/t² as the derivative of something. Let me note that d/dt [ (sin t)/t ] = (t cos t - sin t)/t². Hmm, that's similar but not exactly our integrand. Let's see: (t - sin t)/t² = 1/t - sin t / t². Let me think if this can be expressed as a derivative. Let's compute d/dt [ (1 - cos t)/t ] = (sin t)/t - (1 - cos t)/t². Not quite. Alternatively, d/dt [ something else ].

Alternatively, consider integrating 1/t e^{-t} and sin t / t² e^{-t} separately. But as before, the first integral is divergent. However, maybe the difference converges. Let me check the behavior as t approaches 0. For small t, t - sin t ≈ t - (t - t^3/6) = t^3/6. So (t - sin t)/t² ≈ t/6. Multiply by e^{-t} ≈1, so the integrand behaves like t/6, which is integrable near 0. As t approaches infinity, the integrand is (t - sin t)/t² e^{-t} ≈ (t)/t² e^{-t} = e^{-t}/t, which decays exponentially. So the integral is convergent. 

But how to compute it analytically? Let's consider expanding sin t into its Taylor series. So sin t = Σ_{n=0}^∞ (-1)^n t^{2n+1}/(2n+1)! ). Then t - sin t = Σ_{n=1}^∞ (-1)^{n+1} t^{2n+1}/(2n+1)! ). Then (t - sin t)/t² = Σ_{n=1}^∞ (-1)^{n+1} t^{2n-1}/(2n+1)! ). Then multiply by e^{-t} and integrate term by term. 

So the integral becomes Σ_{n=1}^∞ [ (-1)^{n+1} / (2n+1)! ) ] ∫₀^∞ t^{2n -1} e^{-t} dt. The integral ∫₀^∞ t^{2n -1} e^{-t} dt is the Gamma function Γ(2n) = (2n -1)! ). So the sum becomes Σ_{n=1}^∞ [ (-1)^{n+1} / (2n+1)! ) ] * (2n -1)! ). Simplify the terms: (2n -1)! / (2n +1)! ) = 1/(2n(2n +1)). So the sum is Σ_{n=1}^∞ [ (-1)^{n+1} / (2n(2n +1)) ].

So the integral is equal to Σ_{n=1}^∞ [ (-1)^{n+1} / (2n(2n +1)) ]. Let's compute this series. Let me write the terms:

For n=1: (-1)^{2} / (2*1*(2*1 +1)) = 1/(2*3) = 1/6

n=2: (-1)^3 / (4*5) = -1/20

n=3: 1/(6*7) = 1/42

n=4: -1/(8*9) = -1/72

And so on. So the series is 1/6 - 1/20 + 1/42 - 1/72 + ... 

This is an alternating series. To sum it, perhaps express it in terms of known series. Let me consider writing 1/(2n(2n+1)) as partial fractions. Let's see:

1/(2n(2n+1)) = A/(2n) + B/(2n+1). Solving for A and B:

1 = A(2n+1) + B(2n)

Set n = -1/2: 1 = A(0) + B(-1) => B = -1

Set n=0: 1 = A(1) + B(0) => A=1

So 1/(2n(2n+1)) = 1/(2n) - 1/(2n+1). Therefore, the sum becomes Σ_{n=1}^∞ (-1)^{n+1} [1/(2n) - 1/(2n+1)].

Split the sum into two:

Σ_{n=1}^∞ (-1)^{n+1}/(2n) - Σ_{n=1}^∞ (-1)^{n+1}/(2n+1)

Let’s compute each series separately. 

First series: S1 = Σ_{n=1}^∞ (-1)^{n+1}/(2n) = (1/2) Σ_{n=1}^∞ (-1)^{n+1}/n. The sum Σ_{n=1}^∞ (-1)^{n+1}/n is ln 2. So S1 = (1/2) ln 2.

Second series: S2 = Σ_{n=1}^∞ (-1)^{n+1}/(2n+1). Let's write this as Σ_{k=0}^∞ (-1)^{k}/(2k+3) where k = n-1. Wait, alternatively, note that Σ_{n=0}^∞ (-1)^n/(2n+1) = π/4. But our sum starts at n=1. So S2 = Σ_{n=1}^∞ (-1)^{n+1}/(2n+1) = - Σ_{n=1}^∞ (-1)^n/(2n+1) = - [ Σ_{n=0}^∞ (-1)^n/(2n+1) - (-1)^0/(2*0 +1) ] = - [ π/4 - 1 ] = 1 - π/4.

Wait, let me verify that. The sum from n=0 to ∞ of (-1)^n/(2n+1) is indeed π/4. So the sum from n=1 to ∞ is π/4 - 1. Therefore, S2 = - (π/4 -1) = 1 - π/4. But wait, in our case, the sign is (-1)^{n+1}/(2n+1). Let me check:

Σ_{n=1}^∞ (-1)^{n+1}/(2n+1) = - Σ_{n=1}^∞ (-1)^n/(2n+1) = - [ Σ_{n=0}^∞ (-1)^n/(2n+1) - (-1)^0/(2*0 +1) ] = - [ π/4 -1 ] = 1 - π/4. Yes, that's correct.

Therefore, the original sum is S1 - S2 = (1/2) ln 2 - (1 - π/4) = (1/2) ln 2 -1 + π/4. Wait, no: S1 is (1/2) ln 2? Wait, no. S1 is (1/2) ln 2. Then S1 = (1/2) ln 2, and S2 = 1 - π/4. So the total sum is S1 - S2 = (1/2) ln 2 - (1 - π/4) = (1/2) ln 2 -1 + π/4.

Therefore, the integral equals (1/2) ln 2 -1 + π/4. Let me compute this expression. 

First, compute each term:

(1/2) ln 2 ≈ 0.5 * 0.69314718056 ≈ 0.34657359028

Then subtract 1: 0.34657359028 -1 ≈ -0.65342640972

Then add π/4 ≈ 0.7853981634. So total ≈ -0.65342640972 + 0.7853981634 ≈ 0.13197175368. 

So the integral is approximately 0.13197. But let's check the exact expression. 

Wait, the integral is (1/2) ln 2 -1 + π/4. Let me write that as π/4 -1 + (ln 2)/2. 

Alternatively, combining constants: π/4 -1 + (ln 2)/2. 

But let me verify the steps again to ensure no mistakes. 

We had the integral = Σ_{n=1}^∞ [ (-1)^{n+1}/(2n(2n+1)) ] = Σ_{n=1}^∞ (-1)^{n+1} [1/(2n) -1/(2n+1) ] = Σ_{n=1}^∞ (-1)^{n+1}/(2n) - Σ_{n=1}^∞ (-1)^{n+1}/(2n+1) = S1 - S2.

S1 = Σ_{n=1}^∞ (-1)^{n+1}/(2n) = (1/2) Σ_{n=1}^∞ (-1)^{n+1}/n = (1/2) ln 2. Correct.

S2 = Σ_{n=1}^∞ (-1)^{n+1}/(2n+1) = - Σ_{n=1}^∞ (-1)^n/(2n+1) = - [ Σ_{n=0}^∞ (-1)^n/(2n+1) - (-1)^0/(1) ] = - [ π/4 -1 ] = 1 - π/4. Correct.

Therefore, integral = S1 - S2 = (1/2) ln 2 - (1 - π/4) = (1/2) ln 2 -1 + π/4. 

Yes, that's correct. So the exact answer is π/4 -1 + (ln 2)/2. 

Alternatively, we can write this as (π/4) + (ln 2)/2 -1. 

Now, let's compute the numerical approximation. 

Compute each term:

π ≈ 3.1415926536, so π/4 ≈ 0.7853981634

ln 2 ≈ 0.69314718056, so (ln 2)/2 ≈ 0.3465735903

Then add them: 0.7853981634 + 0.3465735903 = 1.1319717537

Subtract 1: 1.1319717537 -1 = 0.1319717537

So the numerical value is approximately 0.1319717537, which rounds to 0.1319717537 when rounded to 10 decimal places. 

Therefore, the exact answer is π/4 + (ln 2)/2 -1, and the numerical approximation is approximately 0.1319717537. 

Let me check if there's another way to express the exact answer. Maybe combining terms. Let's see:

π/4 -1 + (ln 2)/2 = (π/4) + (ln 2)/2 -1. Alternatively, factor out 1/2: (π/4) -1 + (ln 2)/2. But I think the expression is simplest as π/4 + (ln 2)/2 -1. 

Alternatively, we can write it as (π/4 -1) + (ln 2)/2. Either way, that's the exact answer. 

So the final answer in LaTeX is \boxed{\frac{\pi}{4} + \frac{\ln 2}{2} - 1} and the numerical approximation is approximately 0.1319717537.
</think>

{"answer": "\\frac{\\pi}{4} + \\frac{\\ln 2}{2} - 1", "numerical_answer": 0.1319717537}