Let's solve the integral:
\[
I = \int_0^1 \sqrt[3]{x} \left\lfloor \frac{1}{\sqrt[3]{x}} \right\rfloor \, dx
\]

**Step 1: Substitution and setting up intervals**

Let \( y = \sqrt[3]{x} \implies x = y^3, \ dx = 3y^2 dy \).
When \( x = 0 \), \( y = 0 \).
When \( x = 1 \), \( y = 1 \).

Also,
\[
\left\lfloor \frac{1}{\sqrt[3]{x}} \right\rfloor = \lfloor y^{-1} \rfloor
\]

Substituting,
\[
I = \int_{y=0}^{y=1} y \lfloor y^{-1} \rfloor 3y^2 dy = 3 \int_0^1 y^3 \lfloor y^{-1} \rfloor dy
\]

**Step 2: Split into intervals**

For integer \( n \geq 1 \),
\[
\frac{1}{n+1} < y \leq \frac{1}{n} \implies n < y^{-1} \leq n+1 \implies \lfloor y^{-1} \rfloor = n
\]
So, on interval \( y \in \left( \frac{1}{n+1}, \frac{1}{n} \right] \), \( \lfloor y^{-1} \rfloor = n \).

For each \( n \geq 1 \),
\[
I = 3 \sum_{n=1}^\infty \int_{1/(n+1)}^{1/n} n y^3 dy = 3 \sum_{n=1}^\infty n \int_{1/(n+1)}^{1/n} y^3 dy
\]

Compute the inner integral:
\[
\int y^3 dy = \frac{y^4}{4}
\]
So,
\[
I = 3 \sum_{n=1}^\infty n \left[ \frac{y^4}{4} \bigg|_{y=1/(n+1)}^{y=1/n} \right] = \frac{3}{4} \sum_{n=1}^\infty n \left( \frac{1}{n^4} - \frac{1}{(n+1)^4} \right)
\]

**Step 3: Simplify the sum**

\[
n \left( \frac{1}{n^4} - \frac{1}{(n+1)^4} \right) = \frac{1}{n^3} - \frac{n}{(n+1)^4}
\]
So,
\[
I = \frac{3}{4} \left( \sum_{n=1}^\infty \frac{1}{n^3} - \sum_{n=1}^\infty \frac{n}{(n+1)^4} \right)
\]

Examine the second term:
\[
\sum_{n=1}^\infty \frac{n}{(n+1)^4}
\]
Let \( m = n+1 \implies n = m-1 \), as \( n \) runs from 1 to \( \infty \), \( m \) runs from 2 to \( \infty \).
So,
\[
\sum_{n=1}^\infty \frac{n}{(n+1)^4} = \sum_{m=2}^\infty \frac{m-1}{m^4} = \sum_{m=2}^\infty \frac{1}{m^3} - \frac{1}{m^4}
\]

**Step 4: Plug everything in**

Back to the main sum:
\[
I = \frac{3}{4} \left[ \sum_{n=1}^\infty \frac{1}{n^3} - \left( \sum_{m=2}^\infty \frac{1}{m^3} - \frac{1}{m^4} \right) \right]
\]
\[
= \frac{3}{4} \left[ \frac{1}{1^3} + \sum_{n=2}^\infty \frac{1}{n^3} - \left( \sum_{m=2}^\infty \frac{1}{m^3} - \frac{1}{m^4} \right) \right]
\]
\[
= \frac{3}{4} \left[ 1 + \sum_{n=2}^\infty \frac{1}{n^3} - \sum_{m=2}^\infty \frac{1}{m^3} + \sum_{m=2}^\infty \frac{1}{m^4} \right]
\]
\[
= \frac{3}{4} \left[ 1 + \sum_{m=2}^\infty \frac{1}{m^4} \right]
\]

But,
\[
\sum_{n=2}^\infty \frac{1}{n^4} = \zeta(4) - 1
\]
So,
\[
I = \frac{3}{4} \left[ 1 + \zeta(4) - 1 \right] = \frac{3}{4} \zeta(4)
\]

We know \( \zeta(4) = \frac{\pi^4}{90} \), so
\[
I = \frac{3}{4} \cdot \frac{\pi^4}{90} = \frac{\pi^4}{120}
\]

**Step 5: Numerical value**

\[
\pi^4 \approx 97.40909103400243723644033
\]
So,
\[
I \approx \frac{97.40909103400243723644}{120} = 0.8117424253
\]

**Final answer:**

```json
{"answer": "\\frac{\\pi^4}{120}", "numerical_answer": "0.8117424253"}
```