Let's denote the integral as:
\[
I = \int_{0}^{1} \frac{1}{1+x^2} \arctan\left(x^{3+\sqrt{8}}\right) \, dx
\]

### Step 1: Substitution

Let’s try to find a symmetry or substitution. Observe that:
Let \( \alpha = 3+\sqrt{8} \), so the integral becomes
\[
I = \int_{0}^{1} \frac{1}{1+x^2} \arctan\left(x^{\alpha}\right) dx
\]

Let’s consider substituting \( x \to 1/x \) and try to combine the integral with itself.

Let’s compute:
Let \( x = \tan \theta \), for \( x \in [0,1] \), \( \theta \in [0, \frac{\pi}{4}] \).

Then,
\[
dx = \sec^2 \theta\, d\theta;\quad x^2 = \tan^2 \theta; \quad 1 + x^2 = 1 + \tan^2 \theta = \sec^2 \theta
\]

So:
\[
\frac{1}{1+x^2} dx = d\theta
\]

Thus, the integral is
\[
I = \int_{0}^{\frac{\pi}{4}} \arctan\left( [\tan \theta]^{\alpha} \right) d\theta
\]
\[
= \int_{0}^{\frac{\pi}{4}} \arctan\left( \tan^{\alpha} \theta \right) d\theta
\]

Now, recall that for \( \theta \in [0, \frac{\pi}{4}] \), \( \tan \theta \in [0,1] \), and thus \( \tan^{\alpha} \theta \) also in \([0,1]\), so \( \arctan(\tan^{\alpha} \theta) \) is in \([0, \frac{\pi}{4}]\).

Now, consider the following substitution on \( \theta \):

Let \( \theta' = \frac{\pi}{4} - \theta \), thus when \( \theta = 0 \), \( \theta' = \frac{\pi}{4} \), and when \( \theta = \frac{\pi}{4} \), \( \theta' = 0 \).
Thus, the limits are swapped. Also,
\[
\tan(\theta') = \tan(\frac{\pi}{4} - \theta) = \frac{1 - \tan\theta}{1 + \tan\theta}
\]

But this seems complicated. Let's try instead another approach.

### Step 2: Try Integration by Parts

Let us attempt integrating by parts, with
\[
u = \arctan \left( x^{\alpha} \right),\quad dv = \frac{1}{1+x^2} dx
\]
then
\[
du = \frac{1}{1 + x^{2\alpha}} \cdot \alpha x^{\alpha-1} dx,\quad v = \arctan x
\]

Thus:
\[
I = u v \bigg|_{x=0}^{x=1} - \int_{0}^{1} v\, du
\]
\[
= \left. \arctan(x^{\alpha}) \arctan x \right|_{0}^{1} - \int_{0}^{1} \arctan x \cdot \frac{\alpha x^{\alpha-1}}{1 + x^{2\alpha}} dx
\]

Compute the boundary terms:

At \( x = 1 \), \( \arctan(1^{\alpha}) = \arctan(1) = \frac{\pi}{4} \), \( \arctan 1 = \frac{\pi}{4} \), so the product is \( \frac{\pi}{4} \cdot \frac{\pi}{4} = \frac{\pi^2}{16} \).

At \( x = 0 \), \( \arctan(0^{\alpha}) = \arctan(0) = 0 \), \( \arctan 0 = 0 \), so the product is 0.

Therefore,
\[
I = \frac{\pi^2}{16} - \alpha \int_{0}^{1} \frac{ x^{\alpha - 1} \arctan x }{1 + x^{2\alpha}} dx
\]

Set
\[
J = \int_{0}^{1} \frac{ x^{\alpha - 1} \arctan x }{1 + x^{2\alpha}} dx
\]

### Step 3: Substitute in J

Let’s try to change variables in \( J \):

Let \( y = x^{\alpha} \implies x = y^{1/\alpha} \implies dx = \frac{1}{\alpha} y^{\frac{1}{\alpha}-1} dy \).

When \( x = 0 \implies y = 0 \), when \( x = 1 \implies y = 1 \).

Calculate \( x^{\alpha-1} = x^{\alpha} x^{-1} = y x^{-1} = y y^{-1/\alpha} = y^{1-1/\alpha} \).
Calculate \( \arctan x = \arctan (y^{1/\alpha}) \).

Thus:
\[
J = \int_{x=0}^{x=1} \frac{ x^{\alpha-1} \arctan x }{1 + x^{2\alpha}} dx
= \int_{y=0}^{y=1} \frac{ y^{1-1/\alpha} \arctan(y^{1/\alpha}) }{1 + y^2} \cdot \frac{1}{\alpha} y^{\frac{1}{\alpha} - 1} dy
\]
Now,
\[
y^{1 - 1/\alpha + \frac{1}{\alpha} - 1} = y^0 = 1
\]
So,
\[
J = \frac{1}{\alpha} \int_{0}^{1} \frac{ \arctan(y^{1/\alpha}) }{1 + y^2} dy
\]

Let’s denote \( \beta = 1/\alpha \).

Therefore,
\[
J = \frac{1}{\alpha} \int_{0}^{1} \frac{ \arctan(y^{\beta}) }{1 + y^2} dy
\]

But our original \( I \) is:
\[
I = \frac{\pi^2}{16} - \alpha J
= \frac{\pi^2}{16} - \alpha \cdot \frac{1}{\alpha} \int_{0}^{1} \frac{ \arctan(y^{1/\alpha}) }{1 + y^2} dy
= \frac{\pi^2}{16} - \int_{0}^{1} \frac{ \arctan(y^{1/\alpha}) }{1 + y^2} dy
\]

Note that this is of the same form as our original integral, **but with the exponent replaced with \( 1/\alpha \) instead of \( \alpha \)**. Thus, if we call
\[
I(\gamma) = \int_0^1 \frac{1}{1+x^2} \arctan(x^{\gamma}) dx
\]
then
\[
I(\gamma) = \frac{\pi^2}{16} - I(1/\gamma)
\]
Thus,
\[
I(\gamma) + I(1/\gamma) = \frac{\pi^2}{16}
\]

Back to our problem:
\[
I = I(\alpha), \quad \alpha = 3+\sqrt{8}
\]
Note \( 1/\alpha = 3-\sqrt{8} \) because \( (3+\sqrt{8})(3-\sqrt{8}) = 9-8 = 1 \), so indeed \( 1/\alpha = 3-\sqrt{8} \).

Therefore,
\[
I(3+\sqrt{8}) + I(3-\sqrt{8}) = \frac{\pi^2}{16}
\]
But by the symmetry, \( I(3+\sqrt{8}) = I(3-\sqrt{8}) \) because both exponents are reciprocals and the relation is symmetric.

Thus,
\[
2I(3+\sqrt{8}) = \frac{\pi^2}{16} \implies I(3+\sqrt{8}) = \frac{\pi^2}{32}
\]

---

### Step 4: Numerical Evaluation

\[
\frac{\pi^2}{32}
\]
Calculate its value:
\[
\pi^2 = 9.8696044011
\]
So,
\[
\frac{\pi^2}{32} = \frac{9.8696044011}{32} \approx 0.3084251375
\]

---

### Step 5: Final Answer in JSON

```json
{"answer": "\\frac{\\pi^2}{32}", "numerical_answer": "0.3084251375"}
```