# Evaluating $\int_{0}^{1}x^{-1/2}(1-x)^{-1/2}T_{4}\left(\sqrt{x(1-x)}\right)dx$

First, I need to recall that $T_4(x)$ is the 4th Chebyshev polynomial of the first kind, which can be expressed as:
$$T_4(x) = 8x^4 - 8x^2 + 1$$

## Step 1: Express the integrand in terms of $T_4\left(\sqrt{x(1-x)}\right)$
Let's substitute $u = \sqrt{x(1-x)}$ into the Chebyshev polynomial:
$$T_4\left(\sqrt{x(1-x)}\right) = 8(x(1-x))^2 - 8(x(1-x)) + 1$$
$$T_4\left(\sqrt{x(1-x)}\right) = 8x^2(1-x)^2 - 8x(1-x) + 1$$
$$T_4\left(\sqrt{x(1-x)}\right) = 8x^2(1-2x+x^2) - 8x(1-x) + 1$$
$$T_4\left(\sqrt{x(1-x)}\right) = 8x^2 - 16x^3 + 8x^4 - 8x + 8x^2 + 1$$
$$T_4\left(\sqrt{x(1-x)}\right) = 8x^4 - 16x^3 + 16x^2 - 8x + 1$$

## Step 2: Set up the integral with this expansion
$$\int_{0}^{1}x^{-1/2}(1-x)^{-1/2}T_{4}\left(\sqrt{x(1-x)}\right)dx$$
$$= \int_{0}^{1}x^{-1/2}(1-x)^{-1/2}(8x^4 - 16x^3 + 16x^2 - 8x + 1)dx$$
$$= 8\int_{0}^{1}x^{-1/2+4}(1-x)^{-1/2}dx - 16\int_{0}^{1}x^{-1/2+3}(1-x)^{-1/2}dx + 16\int_{0}^{1}x^{-1/2+2}(1-x)^{-1/2}dx - 8\int_{0}^{1}x^{-1/2+1}(1-x)^{-1/2}dx + \int_{0}^{1}x^{-1/2}(1-x)^{-1/2}dx$$
$$= 8\int_{0}^{1}x^{7/2}(1-x)^{-1/2}dx - 16\int_{0}^{1}x^{5/2}(1-x)^{-1/2}dx + 16\int_{0}^{1}x^{3/2}(1-x)^{-1/2}dx - 8\int_{0}^{1}x^{1/2}(1-x)^{-1/2}dx + \int_{0}^{1}x^{-1/2}(1-x)^{-1/2}dx$$

## Step 3: Use the beta function
I'll use the beta function formula: $\int_{0}^{1}x^{\alpha-1}(1-x)^{\beta-1}dx = B(\alpha,\beta) = \frac{\Gamma(\alpha)\Gamma(\beta)}{\Gamma(\alpha+\beta)}$

For each term:
1. $\int_{0}^{1}x^{7/2}(1-x)^{-1/2}dx = B(9/2,1/2) = \frac{\Gamma(9/2)\Gamma(1/2)}{\Gamma(5)}$
2. $\int_{0}^{1}x^{5/2}(1-x)^{-1/2}dx = B(7/2,1/2) = \frac{\Gamma(7/2)\Gamma(1/2)}{\Gamma(4)}$
3. $\int_{0}^{1}x^{3/2}(1-x)^{-1/2}dx = B(5/2,1/2) = \frac{\Gamma(5/2)\Gamma(1/2)}{\Gamma(3)}$
4. $\int_{0}^{1}x^{1/2}(1-x)^{-1/2}dx = B(3/2,1/2) = \frac{\Gamma(3/2)\Gamma(1/2)}{\Gamma(2)}$
5. $\int_{0}^{1}x^{-1/2}(1-x)^{-1/2}dx = B(1/2,1/2) = \frac{\Gamma(1/2)\Gamma(1/2)}{\Gamma(1)}$

We know that:
- $\Gamma(1/2) = \sqrt{\pi}$
- $\Gamma(n+1) = n\Gamma(n)$
- $\Gamma(1) = 1$

Computing these values:
- $\Gamma(9/2) = \frac{7!}{2^7}\sqrt{\pi} = \frac{5040}{128}\sqrt{\pi} = \frac{315}{8}\sqrt{\pi}$
- $\Gamma(7/2) = \frac{5!}{2^5}\sqrt{\pi} = \frac{120}{32}\sqrt{\pi} = \frac{15}{4}\sqrt{\pi}$
- $\Gamma(5/2) = \frac{3!}{2^3}\sqrt{\pi} = \frac{6}{8}\sqrt{\pi} = \frac{3}{4}\sqrt{\pi}$
- $\Gamma(3/2) = \frac{1}{2}\sqrt{\pi}$
- $\Gamma(5) = 24$
- $\Gamma(4) = 6$
- $\Gamma(3) = 2$
- $\Gamma(2) = 1$

Now, let's compute each beta function:
1. $B(9/2,1/2) = \frac{\Gamma(9/2)\Gamma(1/2)}{\Gamma(5)} = \frac{\frac{315}{8}\sqrt{\pi} \cdot \sqrt{\pi}}{24} = \frac{315\pi}{192}$
2. $B(7/2,1/2) = \frac{\Gamma(7/2)\Gamma(1/2)}{\Gamma(4)} = \frac{\frac{15}{4}\sqrt{\pi} \cdot \sqrt{\pi}}{6} = \frac{15\pi}{24}$
3. $B(5/2,1/2) = \frac{\Gamma(5/2)\Gamma(1/2)}{\Gamma(3)} = \frac{\frac{3}{4}\sqrt{\pi} \cdot \sqrt{\pi}}{2} = \frac{3\pi}{8}$
4. $B(3/2,1/2) = \frac{\Gamma(3/2)\Gamma(1/2)}{\Gamma(2)} = \frac{\frac{1}{2}\sqrt{\pi} \cdot \sqrt{\pi}}{1} = \frac{\pi}{2}$
5. $B(1/2,1/2) = \frac{\Gamma(1/2)\Gamma(1/2)}{\Gamma(1)} = \frac{\sqrt{\pi} \cdot \sqrt{\pi}}{1} = \pi$

## Step 4: Substitute these values back into our integral
$$\int_{0}^{1}x^{-1/2}(1-x)^{-1/2}T_{4}\left(\sqrt{x(1-x)}\right)dx$$
$$= 8 \cdot \frac{315\pi}{192} - 16 \cdot \frac{15\pi}{24} + 16 \cdot \frac{3\pi}{8} - 8 \cdot \frac{\pi}{2} + \pi$$
$$= \frac{8 \cdot 315\pi}{192} - \frac{16 \cdot 15\pi}{24} + \frac{16 \cdot 3\pi}{8} - \frac{8\pi}{2} + \pi$$
$$= \frac{2520\pi}{192} - \frac{240\pi}{24} + \frac{48\pi}{8} - 4\pi + \pi$$

Let's simplify:
$$\frac{2520\pi}{192} = \frac{105\pi}{8}$$
$$\frac{240\pi}{24} = 10\pi$$
$$\frac{48\pi}{8} = 6\pi$$

So our integral becomes:
$$\frac{105\pi}{8} - 10\pi + 6\pi - 4\pi + \pi$$
$$= \frac{105\pi}{8} - 7\pi$$
$$= \frac{105\pi - 56\pi}{8}$$
$$= \frac{49\pi}{8}$$

## Step 5: Calculate numerical value
The numerical value of $\frac{49\pi}{8}$ is:
$\frac{49 \times 3.14159265359...}{8} = 19.2422711634...$

Rounded to 10 decimal places: 19.2422711634

## Final Answer
The definite integral $\int_{0}^{1}x^{-1/2}(1-x)^{-1/2}T_{4}\left(\sqrt{x(1-x)}\right)dx = \frac{49\pi}{8}$

{"answer": "\\frac{49\\pi}{8}", "numerical_answer": "19.2422711634"}