<think>
Okay, let's tackle this integral step by step. The problem is to compute the definite integral from 0 to infinity of x^(2-1)e^(-1.0x²) times H₂(1.0x) dx. First, I need to make sure I understand all the components here. 

So, the integrand is x^(2-1) which simplifies to x, multiplied by e^(-x²) and the Hermite polynomial H₂(1.0x). Wait, the Hermite polynomials are usually denoted as H_n(x), and here it's H₂(1.0x). Let me recall the definition of Hermite polynomials. The physicists' Hermite polynomials are given by H_n(x) = (-1)^n e^{x²} d^n/dx^n e^{-x²}. The first few are H₀(x) = 1, H₁(x) = 2x, H₂(x) = 4x² - 2. So H₂(ax) would be 4(ax)² - 2. In this case, a is 1.0, so H₂(x) is 4x² - 2. Therefore, H₂(1.0x) is 4*(1.0x)^2 - 2 = 4x² - 2. So substituting that into the integrand, the integral becomes ∫₀^∞ x e^{-x²} (4x² - 2) dx.

Wait, let me check that again. The original integral is ∫₀^∞ x^{2-1} e^{-1.0x²} H_2(1.0x) dx. Since 2-1 is 1, so x^1, which is x. The exponential term is e^{-x²} because 1.0x² is just x². And H₂(1.0x) is H₂(x) scaled by 1.0, which as I said is 4x² - 2. So substituting that in, the integrand becomes x * e^{-x²} * (4x² - 2). So expanding that, the integral becomes ∫₀^∞ (4x³ - 2x) e^{-x²} dx.

Now, I can split this into two separate integrals: 4∫₀^∞ x³ e^{-x²} dx minus 2∫₀^∞ x e^{-x²} dx. Let's compute each integral separately.

Starting with the first integral: ∫ x³ e^{-x²} dx from 0 to ∞. Let me recall that the integral of x^n e^{-x²} from 0 to ∞ is (1/2) Γ((n+1)/2), where Γ is the gamma function. For n being an integer, if n is even, say n=2m, then Γ(m + 1/2) can be expressed in terms of factorials, but here n=3, which is odd. So n=3, so (n+1)/2 = 2), so Γ(2) = 1! = 1. Wait, wait, Γ(k) = (k-1)! for integer k. So if (n+1)/2 is 2, then Γ(2) = 1! = 1. Wait, ∫₀^∞ x³ e^{-x²} dx = (1/2) Γ(2) = (1/2)(1!) = 1/2. Wait, but let me check that again. Let me compute the integral directly. Let’s make substitution u = x², so du = 2x dx. Then x³ e^{-x²} dx = x² * x e^{-x²} dx. Let u = x², so x = u^{1/2}, du = 2x dx => x dx = du/2. Then x³ e^{-x²} dx = u * (du/2) e^{-u} = (u e^{-u} du)/2. So the integral becomes (1/2) ∫₀^∞ u e^{-u} du. The integral of u e^{-u} from 0 to ∞ is Γ(2) = 1! = 1. So the integral is (1/2)(1) = 1/2. So that's correct. So the first integral is 4*(1/2) = 2.

Now the second integral: ∫₀^∞ x e^{-x²} dx. Let's compute this. Again, substitution u = x², du = 2x dx, so x dx = du/2. The integral becomes (1/2) ∫₀^∞ e^{-u} du = (1/2)(-e^{-u}) from 0 to ∞ = (1/2)(0 - (-1)) = 1/2. So the second integral is -2*(1/2) = -1.

Adding both results: 2 - 1 = 1. So the exact value of the integral is 1.

Wait, that seems straightforward, but let me verify again. Let me check the Hermite polynomial substitution again. H₂(x) is 4x² - 2, so H₂(1.0x) is 4x² - 2. Then the integrand is x*(4x² - 2)*e^{-x²} = (4x³ - 2x)e^{-x²}. Then splitting into two integrals: 4∫x³ e^{-x²} dx - 2∫x e^{-x²} dx. The first integral, as computed, is 4)(1/2) = 2. The second integral is (-2)(1/2) = -1. So total is 2 -1 =1. So the exact answer is 1. 

But wait, let me check if there's any possible mistake here. For example, maybe the limits of integration? The original integral is from 0 to infinity, and the substitution for u = x² would have u going from 0 to infinity as x does. So that's correct. The gamma function approach also gives the same result. So I think this is correct. 

Alternatively, maybe there's a different definition of Hermite polynomials. Wait, sometimes the probabilists' Hermite polynomials are different. The physicists' Hermite polynomials are as I mentioned, but the probabilists' are scaled differently. Let me confirm. The physicists' Hermite polynomials H_n(x) are as I described, with H₂(x) = 4x² - 2. The probabilists' use a different scaling, but since the problem uses H_2, which is standard in physics, I think that's correct. So H₂(x) = 4x² - 2. So substituting that in is correct. 

Therefore, the exact answer is 1. The numerical approximation would be 1.0000000000. But let me check with a numerical approximation. Let's compute the integral numerically. Let's take the integrand (4x³ - 2x)e^{-x²} from 0 to infinity. Let's split it into two parts: 4x³ e^{-x²} and -2x e^{-x²}. The integral of 4x³ e^{-x²} from 0 to ∞ is 4*(1/2) = 2. The integral of -2x e^{-x²} is -2*(1/2) = -1. So total is 1. So numerically, it's exactly 1. So the numerical approximation is 1.0000000000. 

Therefore, the final answer is 1, both analytically and numerically. So the JSON output should be {"answer": "1", "numerical_answer": "1.0000000000"}.
</think>

{"answer": "1", "numerical_answer": "1.0000000000"}