
To solve the definite integral \(\int\limits_0^2 x \arcsin\left(\frac{1}{2} \sqrt{x(2-x)}\right)\,dx\), we follow these steps:

### Step 1: Simplify the argument of \(\arcsin\)
First, rewrite \(x(2-x)\) by completing the square:
\[
x(2-x) = 2x - x^2 = 1 - (x-1)^2
\]
Thus, the argument of \(\arcsin\) becomes \(\frac{1}{2}\sqrt{1 - (x-1)^2}\).

### Step 2: Substitution for symmetry
Let \(t = x - 1\), so \(x = t + 1\) and \(dx = dt\). The limits change from \(x=0\) to \(t=-1\) and \(x=2\) to \(t=1\). The integral becomes:
\[
\int_{-1}^1 (t + 1) \arcsin\left(\frac{1}{2}\sqrt{1 - t^2}\right)\,dt
\]
This splits into two integrals:
\[
\int_{-1}^1 t \arcsin\left(\frac{1}{2}\sqrt{1 - t^2}\right)\,dt + \int_{-1}^1 \arcsin\left(\frac{1}{2}\sqrt{1 - t^2}\right)\,dt
\]

### Step 3: Odd function cancellation
The first integral involves an odd function (\(t\)) multiplied by an even function (\(\arcsin\left(\frac{1}{2}\sqrt{1 - t^2}\right)\)), so it integrates to 0 over symmetric limits. We only need to evaluate the second integral:
\[
\int_{-1}^1 \arcsin\left(\frac{1}{2}\sqrt{1 - t^2}\right)\,dt
\]

### Step 4: Integration by parts
Let \(u = \arcsin\left(\frac{1}{2}\sqrt{1 - t^2}\right)\) and \(dv = dt\). Then \(du = \frac{-t}{\sqrt{(1 - t^2)(3 + t^2)}}\,dt\) and \(v = t\). Integration by parts gives:
\[
\left. t \arcsin\left(\frac{1}{2}\sqrt{1 - t^2}\right) \right|_{-1}^1 + \int_{-1}^1 \frac{t^2}{\sqrt{(1 - t^2)(3 + t^2)}}\,dt
\]
The boundary term is 0 (since \(\arcsin(0) = 0\) at \(t = \pm 1\)). The remaining integral is even, so:
\[
2 \int_0^1 \frac{t^2}{\sqrt{(1 - t^2)(3 + t^2)}}\,dt
\]

### Step 5: Trigonometric substitution
Let \(t = \sin\theta\) (\(dt = \cos\theta\,d\theta\)), so \(\sqrt{1 - t^2} = \cos\theta\) and the integral becomes:
\[
2 \int_0^{\pi/2} \frac{\sin^2\theta}{\sqrt{3 + \sin^2\theta}}\,d\theta
\]
Using \(3 + \sin^2\theta = 4 - \cos^2\theta\) and substituting \(u = \cos\theta\) (\(du = -\sin\theta\,d\theta\)), we rewrite the integral as:
\[
2 \int_0^1 \frac{1 - u^2}{\sqrt{4 - u^2}}\,du
\]

### Step 6: Evaluate the integral
Split the integrand:
\[
\frac{1 - u^2}{\sqrt{4 - u^2}} = \sqrt{4 - u^2} - \frac{3}{\sqrt{4 - u^2}}
\]
Integrate term-by-term:
\[
\int_0^1 \sqrt{4 - u^2}\,du = \left[\frac{u}{2}\sqrt{4 - u^2} + 2\arcsin\left(\frac{u}{2}\right)\right]_0^1 = \frac{\sqrt{3}}{2} + \frac{\pi}{3}
\]
\[
\int_0^1 \frac{1}{\sqrt{4 - u^2}}\,du = \left[\arcsin\left(\frac{u}{2}\right)\right]_0^1 = \frac{\pi}{6}
\]
Combining these results:
\[
2 \left( \left(\frac{\sqrt{3}}{2} + \frac{\pi}{3}\right) - 3 \cdot \frac{\pi}{6} \right) = \sqrt{3} - \frac{\pi}{3}
\]

### Numerical Approximation
The exact result is \(\sqrt{3} - \frac{\pi}{3}\). Numerically, \(\sqrt{3} \approx 1.73205080757\) and \(\frac{\pi}{3} \approx 1.04719755120\), so:
\[
\sqrt{3} - \frac{\pi}{3} \approx 0.68485325637
\]

{"answer": "\(\sqrt{3} - \frac{\pi}{3}\)", "numerical_answer": "0.6848532564"}