<think>
Okay, let's tackle this integral step by step. The integral given is ∫₀¹ x^(-3/4)(1 - x)^(-1/4) [1 - √(x(1 - x))]^(-2) dx. Hmm, that looks a bit complicated, but maybe there's a substitution that can simplify it.

First, I notice that the integrand has terms x^(-3/4) and (1 - x)^(-1/4), which reminds me of the Beta function. The Beta function is B(p, q) = ∫₀¹ t^(p-1)(1 - t)^(q-1) dt, and it's related to the Gamma function via B(p, q) = Γ(p)Γ(q)/Γ(p+q). But here, there's an extra factor [1 - √(x(1 - x))]^(-2), so it's not a standard Beta function. Maybe a substitution can transform it into a Beta function or something similar known integral.

Let me consider a substitution to simplify the expression inside the brackets. Let’s set t = √(x(1 - x)). Then, t² = x(1 - x). But I need to express x in terms of t. Let's see, solving for x: x(1 - x) = t² → x - x² = t² → x² - x + t² = 0. Using quadratic formula: x = [1 ± √(1 - 4t²)]/2. Hmm, that might complicate things. Maybe another substitution.

Alternatively, let's try a trigonometric substitution. Let’s set x = sin²θ. Then, dx = 2 sinθ cosθ dθ. Let's see how the integrand transforms. When x = 0, θ = 0; x = 1, θ = π/2.

Substituting x = sin²θ, then 1 - x = cos²θ. The integrand becomes:

x^(-3/4) = (sin²θ)^(-3/4) = sin^(-3/2)θ

(1 - x)^(-1/4) = (cos²θ)^(-1/4) = cos^(-1/2)θ

The term [1 - √(x(1 - x))]^2: √(x(1 - x)) = √(sin²θ cos²θ) = sinθ cosθ. So 1 - sinθ cosθ. Therefore, [1 - sinθ cosθ]^(-2).

Putting it all together, the integrand becomes:

sin^(-3/2)θ * cos^(-1/2)θ * [1 - sinθ cosθ]^(-2) * 2 sinθ cosθ dθ

Simplify the terms:

sin^(-3/2)θ * cos^(-1/2)θ * 2 sinθ cosθ = 2 sin^(-3/2 + 1)θ * cos^(-1/2 +1)θ = 2 sin^(-1/2)θ * cos^(1/2)θ

So the integral becomes:

2 ∫₀^{π/2} [sin^(-1/2)θ cos^(1/2)θ] / [1 - sinθ cosθ]^2 dθ

Hmm, not sure if that's better. Let's see if we can manipulate the denominator 1 - sinθ cosθ. Maybe express sinθ cosθ in terms of double angles. Remember that sin2θ = 2 sinθ cosθ, so sinθ cosθ = (1/2) sin2θ. Then 1 - (1/2) sin2θ. So denominator becomes [1 - (1/2) sin2θ]^2. Not sure if that helps.

Alternatively, maybe another substitution. Let’s consider t = θ - something. Alternatively, maybe use substitution u = tanθ. Let’s try u = tanθ, so θ = arctan u, dθ = du/(1 + u²). Then, sinθ = u/√(1 + u²), cosθ = 1/√(1 + u²). Let's substitute:

sin^(-1/2)θ = (u/√(1 + u²))^(-1/2) = u^(-1/2) (1 + u²)^(1/4)

cos^(1/2)θ = (1/√(1 + u²))^(1/2) = (1 + u²)^(-1/4)

So sin^(-1/2)θ cos^(1/2)θ = u^(-1/2) (1 + u²)^(1/4) * (1 + u²)^(-1/4) = u^(-1/2)

Denominator [1 - sinθ cosθ]^2 = [1 - (u/√(1 + u²))(1/√(1 + u²))]^2 = [1 - u/(1 + u²)]^2

So the integral becomes:

2 ∫₀^{∞} u^(-1/2) / [1 - u/(1 + u²)]^2 * [du/(1 + u²)]

Wait, let's check the limits. When θ approaches 0, u = tanθ approaches 0. When θ approaches π/2, u approaches infinity. So the limits are from 0 to ∞. Let's compute the integral:

2 ∫₀^∞ u^(-1/2) / [1 - u/(1 + u²)]² * du/(1 + u²)

Simplify the denominator:

1 - u/(1 + u²) = (1 + u² - u)/(1 + u²) = (u² - u + 1)/(1 + u²)

So denominator squared is (u² - u + 1)^2 / (1 + u²)^2

Therefore, the integrand becomes:

2 * u^(-1/2) * (1 + u²)^2 / (u² - u + 1)^2 * 1/(1 + u²) du

Simplify:

2 u^(-1/2) (1 + u²) / (u² - u + 1)^2 du

So integral is 2 ∫₀^∞ u^(-1/2) (1 + u²)/(u² - u + 1)^2 du

Hmm, this seems complicated. Maybe another substitution. Let's look for a substitution that can simplify the denominator. Let’s note that u² - u + 1 is a quadratic. Maybe complete the square: u² - u + 1 = (u - 1/2)^2 + 3/4. Not sure if that helps. Alternatively, maybe set t = u + something.

Alternatively, consider that the integrand is a rational function multiplied by u^(-1/2). Maybe substitution t = sqrt(u). Let’s set t = √u, so u = t², du = 2t dt. Then, the integral becomes:

2 ∫₀^∞ (t²)^(-1/2) (1 + t⁴)/(t⁴ - t² + 1)^2 * 2t dt

Simplify:

2 * 2 ∫₀^∞ t^(-1) (1 + t⁴)/(t⁴ - t² + 1)^2 * t dt = 4 ∫₀^∞ (1 + t⁴)/(t⁴ - t² + 1)^2 dt

So now the integral is 4 ∫₀^∞ (1 + t⁴)/(t⁴ - t² + 1)^2 dt. Hmm, maybe this is a standard integral or can be expressed via derivatives. Alternatively, partial fractions? But the denominator is a quartic. Let me check if the denominator factors. Let’s see t⁴ - t² + 1. Let’s check for roots. Let’s set z = t², then z² - z + 1 = 0. The discriminant is 1 - 4 = -3, so roots are complex: z = [1 ± i√3]/2. Therefore, t⁴ - t² +1 factors into (t² + at + b)(t² + ct + d). Let me try to factor it. Since the roots are complex, it factors into two quadratics with real coefficients. Let’s suppose t⁴ - t² +1 = (t² + pt + q)(t² + rt + s). Expanding:

t⁴ + (p + r)t³ + (q + s + pr)t² + (ps + rq)t + qs

Compare to t⁴ - t² +1. So coefficients:

p + r = 0

q + s + pr = -1

ps + rq = 0

qs = 1

From p + r = 0, so r = -p.

Then, ps + rq = p s - p q = p(s - q) = 0. So either p=0 or s=q.

If p=0, then r=0, and then q + s = -1, and qs=1. Then solving q + s = -1, qs=1. The quadratic equation would be x² + x +1=0, which has roots complex. But we need real coefficients. So maybe p ≠0, so s = q.

Then, from qs=1 and s=q, so q²=1 → q=1 or q=-1. If q=1, then s=1. Then from q + s + pr = 1 +1 + p*(-p) = 2 - p² = -1 → p²=3 → p=√3 or -√3. Then, the factors would be (t² + √3 t +1)(t² -√3 t +1). Let's check:

(t² + √3 t +1)(t² -√3 t +1) = t⁴ - (√3 t)(√3 t) + ... Wait, expanding:

First term: t²*t² = t⁴

Outer terms: t²*(-√3 t) + t²*(√3 t) = -√3 t³ + √3 t³ = 0

Inner terms: √3 t * t² + (-√3 t)*t² = same as above, zero.

Then cross terms: √3 t * (-√3 t) +1*t² +1*t² +1*1. Wait, maybe better to multiply step by step:

(t² + √3 t +1)(t² -√3 t +1) = t²(t² -√3 t +1) + √3 t(t² -√3 t +1) +1(t² -√3 t +1)

= t⁴ -√3 t³ + t² + √3 t³ - 3 t² + √3 t + t² -√3 t +1

Combine like terms:

t⁴ + (-√3 t³ + √3 t³) + (t² -3 t² + t²) + (√3 t -√3 t) +1

Simplifies to t⁴ - t² +1. Yes! So t⁴ - t² +1 factors into (t² + √3 t +1)(t² -√3 t +1). Therefore, the integral becomes:

4 ∫₀^∞ (1 + t⁴)/[(t² + √3 t +1)(t² -√3 t +1)]² dt

Hmm, that's still complicated, but maybe we can use substitution. Let’s note that 1 + t⁴ = (t⁴ - t² +1) + t². So 1 + t⁴ = (t⁴ - t² +1) + t². Therefore, the integrand becomes [ (t⁴ - t² +1) + t² ] / (t⁴ - t² +1)^2 = 1/(t⁴ - t² +1) + t²/(t⁴ - t² +1)^2

So the integral is 4 ∫₀^∞ [1/(t⁴ - t² +1) + t²/(t⁴ - t² +1)^2] dt

Let’s split the integral into two parts:

4 [ ∫₀^∞ 1/(t⁴ - t² +1) dt + ∫₀^∞ t²/(t⁴ - t² +1)^2 dt ]

Now, perhaps these integrals can be evaluated using substitution or known results. Let’s first compute I1 = ∫₀^∞ 1/(t⁴ - t² +1) dt and I2 = ∫₀^∞ t²/(t⁴ - t² +1)^2 dt.

For I1, since the denominator is t⁴ - t² +1, which we factored as (t² + √3 t +1)(t² -√3 t +1). Maybe use partial fractions. Alternatively, recall that integrals of the form ∫ dx/(x⁴ + ax² +1) can sometimes be evaluated using substitution. Let’s consider substitution t = 1/u. Then, when t →0, u→∞ and vice versa. Let’s see:

I1 = ∫₀^∞ 1/(t⁴ - t² +1) dt. Let’s substitute t = 1/u, dt = -1/u² du. Then, the integral becomes ∫₀^∞ 1/(1/u⁴ -1/u² +1) * (-1/u²) du. Changing limits, when t=0, u=∞; t=∞, u=0. So reversing limits:

I1 = ∫₀^∞ 1/(1/u⁴ -1/u² +1) * (1/u²) du = ∫₀^∞ u²/(1 - u² + u⁴) du = ∫₀^∞ u²/(u⁴ - u² +1) du = I2

So I1 = I2. Therefore, the integral becomes 4(I1 + I2) = 4(2I1) = 8I1. Wait, but that would mean that the original integral is 8I1. But we need to confirm if I1 = I2. Let me check:

Yes, substituting t =1/u in I1 gives I2. Therefore, I1 = I2. Therefore, the integral is 8I1. So we just need to compute I1 and multiply by 8.

So let's compute I1 = ∫₀^∞ 1/(t⁴ - t² +1) dt. To compute this integral, we can use the substitution related to the integral of reciprocal quartic polynomials. Alternatively, use contour integration, but since we need an analytical solution, perhaps use substitution.

Alternatively, note that t⁴ - t² +1 = t⁴ + 2t² +1 -3t² = (t² +1)^2 - (√3 t)^2 = (t² + √3 t +1)(t² -√3 t +1). We already factored this earlier.

Alternatively, use substitution t = tanθ. Let’s try t = tanθ, θ ∈ [0, π/2). Then, dt = sec²θ dθ. Let’s see:

I1 = ∫₀^{π/2} [1/(tan⁴θ - tan²θ +1)] * sec²θ dθ

But tan⁴θ - tan²θ +1 = tan⁴θ +1 - tan²θ. Let’s express in terms of sin and cos:

= (sin⁴θ / cos⁴θ) +1 - (sin²θ / cos²θ) = [sin⁴θ + cos⁴θ - sin²θ cos²θ]/cos⁴θ

Hmm, numerator: sin⁴θ + cos⁴θ - sin²θ cos²θ. Let’s compute:

sin⁴θ + cos⁴θ = (sin²θ + cos²θ)^2 - 2 sin²θ cos²θ = 1 - 2 sin²θ cos²θ

So numerator becomes 1 - 2 sin²θ cos²θ - sin²θ cos²θ = 1 - 3 sin²θ cos²θ

Therefore, denominator of the integrand becomes [1 - 3 sin²θ cos²θ]/cos⁴θ

So the integrand is [cos⁴θ / (1 - 3 sin²θ cos²θ)] * sec²θ dθ = [cos⁴θ / (1 - 3 sin²θ cos²θ)] * (1/cos²θ) dθ = [cos²θ / (1 - 3 sin²θ cos²θ)] dθ

Hmm, not sure if this helps. Maybe another approach. Let’s consider that the integral I1 is a standard form. Let me recall that ∫₀^∞ dx/(x⁴ + ax² +1) can be expressed in terms of π and sqrt terms. Let’s check the general formula.

For the integral ∫₀^∞ dx/(x⁴ + a x² +1), the result is π/(2√(2 + a))). Wait, not sure. Let me verify.

Alternatively, use substitution. Let’s consider x² = y, so x = √y, dx = (1/(2√y)) dy. Then, the integral becomes:

∫₀^∞ (1/(y² + a y +1)) * (1/(2√y)) dy

But this might not help. Alternatively, use the substitution x = 1/t. Then, as before, the integral becomes ∫₀^∞ t²/(t⁴ + a t² +1) dt. Adding the original integral and this, we get:

I + I' = ∫₀^∞ (1 + t²)/(t⁴ + a t² +1) dt. For our case, a = -1. Wait, in our case, the integral is ∫₀^∞ 1/(t⁴ - t² +1) dt. So a = -1.

But I'm not sure. Alternatively, use the substitution t² = z. Then, t = √z, dt = (1/(2√z)) dz. Then, I1 becomes:

∫₀^∞ 1/(z² - z +1) * (1/(2√z)) dz = (1/2) ∫₀^∞ z^{-1/2}/(z² - z +1) dz

This is similar to a Beta function integral but with a quadratic denominator. Maybe use partial fractions with complex roots, but that's complicated.

Alternatively, recall that for ∫₀^∞ x^{m-1}/(1 + x^n) dx = π/(n sin(mπ/n)). But our denominator is a quartic, not a simple x^n +1. Hmm.

Alternatively, use contour integration. But since this is a real integral, maybe use substitution related to trigonometric functions.

Wait, let me recall that the integral of 1/(t⁴ - t² +1) from 0 to ∞ can be evaluated by substitution. Let’s note that t⁴ - t² +1 = t⁴ + 2t² +1 -3t² = (t² +1)^2 - (√3 t)^2 = (t² + √3 t +1)(t² -√3 t +1). So partial fractions:

1/(t⁴ - t² +1) = [A t + B]/(t² + √3 t +1) + [C t + D]/(t² -√3 t +1)

But this might be tedious. Alternatively, use substitution t = e^{iθ} but that's complex analysis. Alternatively, use substitution t = tanθ. Wait, let me try another substitution.

Let’s set u = t - 1/(2t). Wait, not sure. Alternatively, use substitution t = (1 - z)/(1 + z). Not sure.

Alternatively, use the substitution t = sqrt((1 + y)/ (1 - y)). Not sure. Alternatively, use substitution y = t + 1/t. Let’s try that. Let’s set y = t - 1/t. Then, dy = 1 + 1/t² dt. Hmm, not sure. Alternatively, set y = t + 1/t. Then, dy = 1 - 1/t² dt. Not sure.

Alternatively, consider that the function is even, so extend the integral from -infty to infty and use residues. Since the integrand is even, ∫₀^∞ 1/(t⁴ - t² +1) dt = (1/2) ∫_{-∞}^∞ 1/(t⁴ - t² +1) dt. Then, compute the integral via residues.

Let’s try that. The integral is (1/2) ∫_{-∞}^∞ 1/(t⁴ - t² +1) dt. The poles of the integrand are the roots of t⁴ - t² +1 =0. Let’s solve t⁴ - t² +1=0. Let’s set z = t²: z² - z +1=0. Solutions z = [1 ± i√3]/2. So t² = e^{iπ/3} and e^{-iπ/3}. Therefore, the roots are t = ± e^{iπ/6} and t = ± e^{-iπ/6}. So in the upper half-plane, the poles are t = e^{iπ/6} and t = e^{-iπ/6 + iπ} = e^{i5π/6}. Wait, no. Let me compute the roots properly.

The solutions to z² = [1 ± i√3]/2. Let’s write [1 + i√3]/2 = e^{iπ/3}, and [1 - i√3]/2 = e^{-iπ/3}. Therefore, t² = e^{iπ/3} → t = e^{iπ/6}, e^{iπ/6 + iπ} = e^{i7π/6}; and t² = e^{-iπ/3} → t = e^{-iπ/6}, e^{-iπ/6 + iπ} = e^{i5π/6}. So in the upper half-plane, the poles are at t = e^{iπ/6} and t = e^{i5π/6}.

Compute residues at these poles. The residue at t = e^{iπ/6} is lim_{t→e^{iπ/6}} (t - e^{iπ/6}) * 1/(t⁴ - t² +1). Since t⁴ - t² +1 factors as (t² + √3 t +1)(t² -√3 t +1), and t = e^{iπ/6} is a root of t² -√3 t +1=0. Let’s verify:

t² -√3 t +1 = e^{iπ/3} -√3 e^{iπ/6} +1. Let’s compute e^{iπ/3} = cos(π/3) + i sin(π/3) = 1/2 + i (√3/2). √3 e^{iπ/6} = √3 [cos(π/6) + i sin(π/6)] = √3 (√3/2 + i 1/2) = 3/2 + i √3/2. So e^{iπ/3} -√3 e^{iπ/6} +1 = (1/2 + i√3/2) - (3/2 + i√3/2) +1 = (1/2 -3/2 +1) + i(√3/2 -√3/2) = 0 +0i. Yes, correct.

So the denominator can be written as (t² -√3 t +1)(t² +√3 t +1). Therefore, near t = e^{iπ/6}, the denominator is (t - e^{iπ/6})(t - e^{-iπ/6}) (t² +√3 t +1)). Therefore, the residue at t = e^{iπ/6} is 1/[ (e^{iπ/6} - e^{-iπ/6}) ( (e^{iπ/6})² +√3 e^{iπ/6} +1 ) ]

Compute denominator factors:

First factor: e^{iπ/6} - e^{-iπ/6} = 2i sin(π/6) = 2i*(1/2) = i.

Second factor: (e^{iπ/6})² +√3 e^{iπ/6} +1 = e^{iπ/3} +√3 e^{iπ/6} +1. Let’s compute:

e^{iπ/3} = 1/2 + i√3/2

√3 e^{iπ/6} = √3 (√3/2 + i/2) = 3/2 + i√3/2

Adding them with 1:

1/2 + i√3/2 +3/2 + i√3/2 +1 = (1/2 +3/2 +1) + i(√3/2 +√3/2) = 3 + i√3

Therefore, the residue is 1/(i*(3 + i√3)) = 1/(i*(3 + i√3)) = multiply numerator and denominator by (3 - i√3):

= (3 - i√3)/(i*(3 + i√3)(3 - i√3)) = (3 - i√3)/(i*(9 +3)) = (3 - i√3)/(i*12)

= (3 - i√3)/(12i) = multiply numerator and denominator by -i:

= (-i)(3 - i√3)/12 = (-3i + i²√3)/12 = (-3i -√3)/12 = (-√3 -3i)/12

Similarly, the residue at t = e^{i5π/6} is similar. Let’s compute it. The pole is at t = e^{i5π/6}, which is a root of t² +√3 t +1=0. Let’s verify:

t² +√3 t +1 = e^{i5π/3} +√3 e^{i5π/6} +1. Compute e^{i5π/3} = cos(5π/3) + i sin(5π/3) = 1/2 - i√3/2. √3 e^{i5π/6} = √3 [cos(5π/6) + i sin(5π/6)] = √3 (-√3/2 + i/2) = -3/2 + i√3/2. Adding them with 1:

1/2 - i√3/2 -3/2 + i√3/2 +1 = (1/2 -3/2 +1) + i(-√3/2 +√3/2) = 0 +0i. Correct.

So the residue at t = e^{i5π/6} is 1/[ (e^{i5π/6} - e^{-i5π/6}) ( (e^{i5π/6})² -√3 e^{i5π/6} +1 ) ]

First factor: e^{i5π/6} - e^{-i5π/6} = 2i sin(5π/6) = 2i*(1/2) = i.

Second factor: (e^{i5π/6})² -√3 e^{i5π/6} +1 = e^{i5π/3} -√3 e^{i5π/6} +1. Compute:

e^{i5π/3} = 1/2 - i√3/2

-√3 e^{i5π/6} = -√3 (-√3/2 + i/2) = 3/2 - i√3/2

Adding them with 1:

1/2 - i√3/2 +3/2 - i√3/2 +1 = (1/2 +3/2 +1) + i(-√3/2 -√3/2) = 3 - i√3

Therefore, the residue is 1/(i*(3 - i√3)) = 1/(i*(3 - i√3)) = multiply numerator and denominator by (3 + i√3):

= (3 + i√3)/(i*(9 +3)) = (3 + i√3)/(12i) = multiply numerator and denominator by -i:

= (-i)(3 + i√3)/12 = (-3i -i²√3)/12 = (-3i +√3)/12 = (√3 -3i)/12

Now, sum the residues in the upper half-plane:

Residue1 + Residue2 = (-√3 -3i)/12 + (√3 -3i)/12 = [(-√3 +√3) + (-3i -3i)]/12 = (0 -6i)/12 = -i/2

Therefore, the integral over the real line is 2πi * sum of residues = 2πi*(-i/2) = 2πi*(-i)/2 = π. Therefore, the original integral I1 = (1/2)*π = π/2.

Wait, but wait: the integral over the real line is (1/2) ∫_{-infty}^infty ... = I1, and we found that ∫_{-infty}^infty ... = π. Therefore, I1 = π/2.

But wait, no. Wait, the integral we computed via residues is ∫_{-infty}^infty 1/(t⁴ - t² +1) dt = 2πi * sum of residues = π. Therefore, I1 = (1/2) * π = π/2.

But earlier, we had the original integral as 8I1. So the original integral is 8*(π/2) = 4π.

Wait, but let's recap:

Original integral after substitutions became 4*(I1 + I2) = 4*(I1) = 8I1, since I1 = I2. Then, I1 = π/2, so the original integral is 8*(π/2) = 4π.

Therefore, the exact answer is 4π.

But let me verify this result. Let’s check with a numerical approximation. If the exact answer is 4π, then numerically, π is approximately 3.1415926536, so 4π ≈ 12.5663706144.

Let me check with a numerical integration of the original integral. Let’s approximate ∫₀¹ x^(-3/4)(1 - x)^(-1/4)[1 - √(x(1 - x))]^(-2) dx.

But since I can't compute it here, but if the analytical result is 4π, then the numerical should be around 12.5663706144.

Alternatively, let me check with substitution steps again. Let’s see:

We started with the integral, made substitution x = sin²θ, transformed it into 2 ∫ [sin^(-1/2)θ cos^(1/2)θ] / [1 - sinθ cosθ]^2 dθ. Then, through substitutions, we ended up with 8I1, where I1 = π/2. So 8*(π/2) = 4π. Seems correct.

Alternatively, maybe there's a mistake in the substitution steps. Let me check:

Original integral after substitution became 4 ∫₀^∞ (1 + t⁴)/(t⁴ - t² +1)^2 dt. Then, we split into I1 + I2, found I1 = I2 via substitution t =1/u, so integral becomes 8I1. Then, computed I1 = π/2 via residues. So 8*(π/2) =4π. So the exact answer is 4π.

Therefore, the exact answer is 4π, and the numerical approximation is approximately 12.5663706144.

But let me check with another approach. Let’s recall that the original integral is ∫₀¹ x^{-3/4}(1 - x)^{-1/4}[1 - √(x(1 - x)}]^{-2} dx.

Let’s make substitution x = sin²θ, as before. Then, dx = 2 sinθ cosθ dθ. The integral becomes:

∫₀^{π/2} [sin^{-3/2}θ cos^{-1/2}θ] [1 - sinθ cosθ]^{-2} * 2 sinθ cosθ dθ

Simplify the integrand:

2 sin^{-3/2}θ cos^{-1/2}θ * sinθ cosθ = 2 sin^{-1/2}θ cos^{1/2}θ

So integral is 2 ∫₀^{π/2} sin^{-1/2}θ cos^{1/2}θ [1 - sinθ cosθ]^{-2} dθ

Let’s make substitution t = sinθ cosθ. Let’s set t = sinθ cosθ. Then, dt/dθ = cos²θ - sin²θ. But this might not help. Alternatively, set u = sinθ, then du = cosθ dθ. But θ from 0 to π/2, u from 0 to1. Then, cosθ = √(1 - u²). The integral becomes:

2 ∫₀¹ u^{-1/2} (1 - u²)^{1/4} [1 - u√(1 - u²)]^{-2} * [du / √(1 - u²)]

Wait, this seems messy. Alternatively, perhaps another substitution.

Alternatively, note that the integral after substitution is 2 ∫₀^{π/2} [sinθ cosθ]^{-1/2} [1 - sinθ cosθ]^{-2} dθ. Let’s set t = sinθ cosθ. Then, t = (1/2) sin2θ. Let’s set y = 2θ, then θ from 0 to π/2, y from 0 to π. Then, t = (1/2) siny. dt/dy = (1/2) cosy. But this might not help.

Alternatively, use substitution t = sinθ cosθ. Then, t = (1/2) sin2θ. Let’s set u = 2θ, so when θ=0, u=0; θ=π/2, u=π. Then, t = (1/2) sinu. dt = (1/2) cosu du. The integral becomes:

2 ∫₀^{π} [ ( (1/2) sinu )^{-1/2} ] [1 - (1/2) sinu]^{-2} * (1/2) cosu du

But this seems more complicated. Maybe not helpful.

Alternatively, recall that we already did the substitution leading to 4π, which seems plausible. Let’s check with a numerical approximation. For example, compute the integral numerically.

Take x=0.5. Then, x^{-3/4}(1 - x)^{-1/4} = (0.5)^{-3/4}(0.5)^{-1/4} = (0.5)^{-1} = 2. The term [1 - √(0.5*0.5)]^{-2} = [1 - 0.5]^{-2} = (0.5)^{-2} =4. So the integrand at x=0.5 is 2*4=8. But this is just one point. The integral from 0 to1 of a function that peaks at 8 in the middle and has singularities at 0 and1. The exact answer is 4π≈12.566, which seems reasonable.

Alternatively, approximate the integral numerically. Let’s use substitution x = t^4/(1 + t^4). Wait, but this is time-consuming. Alternatively, accept that the analytical result is 4π, and the numerical approximation is approximately 12.5663706144.

Therefore, the final answer is 4π, and the numerical approximation is approximately 12.5663706144.
</think>

{"answer": "4\\pi", "numerical_answer": 12.5663706144}