We wish to evaluate

  I = ∫₀¹ [x²⁄(2 – x²) + √(2x⁄(x + 1))] dx.

It helps to separate the integral into two parts:
  I = I₁ + I₂,
with
  I₁ = ∫₀¹ [x²⁄(2 – x²)] dx  and  I₂ = ∫₀¹ √(2x⁄(x + 1)) dx.

──────────────────────────────
Step 1. Compute I₁.

Begin with
  I₁ = ∫₀¹ [x²⁄(2 – x²)] dx.

Notice that we can rewrite the integrand by “completing” the numerator:
  x²⁄(2 – x²) = –1 + 2⁄(2 – x²).
Indeed,
  2⁄(2 – x²) – 1 = [2 – (2 – x²)]⁄(2 – x²) = x²⁄(2 – x²).

Thus,
  I₁ = ∫₀¹ (–1) dx + 2 ∫₀¹ 1⁄(2 – x²) dx
     = [–x]₀¹ + 2 I₁a
     = –1 + 2 I₁a,
where
  I₁a = ∫₀¹ 1⁄(2 – x²) dx.

To compute I₁a, note that
  ∫ dx⁄(a² – x²) = (1⁄(2a)) ln |(a + x)/(a – x)| + C    (for a > 0).
Here, we have a² = 2 so that a = √2. Therefore,
  I₁a = [1⁄(2√2)] ln |(√2 + x)/(√2 – x)| evaluated from 0 to 1.

Thus,
  I₁a = (1⁄(2√2)) [ ln((√2 + 1)/(√2 – 1)) – ln((√2 + 0)/(√2 – 0)) ]
Since ln((√2)/(√2)) = ln(1) = 0, we have
  I₁a = (1⁄(2√2)) ln((√2 + 1)/(√2 – 1)).

Returning to I₁:
  I₁ = –1 + 2(1⁄(2√2)) ln((√2 + 1)/(√2 – 1))
     = –1 + (1⁄√2) ln((√2 + 1)/(√2 – 1)).

──────────────────────────────
Step 2. Compute I₂.

We have
  I₂ = ∫₀¹ √(2x⁄(x + 1)) dx.
Write the integrand as
  √(2x⁄(x + 1)) = √(2x)⁄√(x + 1).

Make the substitution:
  u = √(x + 1) ⇒ x = u² – 1,
  dx = 2u du.
When x = 0, u = √1 = 1; when x = 1, u = √2.

Now, express the integrand in terms of u:
  √(2x) = √(2(u² – 1)) = √2 √(u² – 1),
  √(x + 1) = u.
Thus,
  I₂ = ∫₍u=1₎^(√2) [ (√2 √(u² – 1))/u ] (2u du)
     = 2√2 ∫₁^(√2) √(u² – 1) du.

Recall the standard integral
  ∫ √(u² – 1) du = (u⁄2)√(u² – 1) – (1⁄2) ln |u + √(u² – 1)| + C.
Therefore,
  I₂ = 2√2 { [ (u⁄2)√(u² – 1) – (1⁄2) ln |u + √(u² – 1)| ]₍u=1₎^(√2) }
     = √2 { [ u√(u² – 1) – ln |u + √(u² – 1)| ]₁^(√2) }.

Evaluate at u = √2:
  u√(u² – 1) = √2·√(2 – 1) = √2,
  ln|u + √(u² – 1)| = ln(√2 + 1).
At u = 1:
  1·√(1 – 1) = 0 and ln|1 + 0| = ln 1 = 0.
Thus,
  I₂ = √2 [ (√2 – ln(√2 + 1)) – 0 ]
     = √2·√2 – √2 ln(√2 + 1)
     = 2 – √2 ln(√2 + 1).

──────────────────────────────
Step 3. Combine I₁ and I₂.

Recall:
  I₁ = –1 + (1⁄√2) ln((√2 + 1)/(√2 – 1))
  I₂ = 2 – √2 ln(√2 + 1)

So,
  I = I₁ + I₂ = [–1 + 2] + [(1⁄√2) ln((√2 + 1)/(√2 – 1)) – √2 ln(√2 + 1)]
     = 1 + (1⁄√2) ln((√2 + 1)/(√2 – 1)) – √2 ln(√2 + 1).

Observe that
  ln((√2 + 1)/(√2 – 1)) = ln(√2 + 1) – ln(√2 – 1).

Thus,
  I = 1 + (1⁄√2)[ln(√2 + 1) – ln(√2 – 1)] – √2 ln(√2 + 1)
     = 1 + (1⁄√2) ln(√2 + 1) – (1⁄√2) ln(√2 – 1) – √2 ln(√2 + 1)
     = 1 – (1⁄√2) ln(√2 – 1) + ln(√2 + 1) (1⁄√2 – √2).

Note that
  1⁄√2 – √2 = (1 – 2)/√2 = –1⁄√2.
Then,
  I = 1 – (1⁄√2) ln(√2 – 1) – (1⁄√2) ln(√2 + 1)
     = 1 – (1⁄√2)[ln(√2 – 1) + ln(√2 + 1)].

But ln(√2 – 1) + ln(√2 + 1) = ln[(√2 – 1)(√2 + 1)] = ln(2 – 1) = ln 1 = 0.

Thus, we obtain
  I = 1.

──────────────────────────────
Step 4. Provide a numerical approximation.

Since the exact result is 1, the numerical approximation is 1.0000000000.

──────────────────────────────
Final Answer in JSON Format:

{"answer": "1", "numerical_answer": "1.0000000000"}