<think>
Okay, let's tackle this integral step by step. The integral given is ∫ from -3/2 to -1/2 of (x⁵ + 5x⁴ + 10x³ + 8x² + x) dx. Hmm, first, I need to compute the antiderivative of each term and then evaluate it at the limits. Let me start by breaking down the integrand into individual terms.

So, the integrand is a polynomial: x⁵ + 5x⁴ + 10x³ + 8x² + x. Integrating term by term should work here. Let's find the antiderivative of each term.

Starting with x⁵. The integral of x^n is (x^(n+1))/(n+1), so for n=5, that becomes (x⁶)/6.

Next term is 5x⁴. The integral would be 5*(x⁵)/5) which simplifies to x⁵.

Third term is 10x³. Integral is 10*(x⁴)/4 = (10/4)x⁴ = (5/2)x⁴.

Fourth term is 8x². Integral is 8*(x³)/3 = (8/3)x³.

Last term is x. Integral is (x²)/2.

Putting all these together, the antiderivative F(x) is:

F(x) = (1/6)x⁶ + x⁵ + (5/2)x⁴ + (8/3)x³ + (1/2)x² + C

Now, since it's a definite integral from -3/2 to -1/2, we need to compute F(-1/2) - F(-3/2).

Let me compute each part step by step. Let's first compute F(-1/2):

Compute each term at x = -1/2:

1. (1/6)(-1/2)^6: (-1/2)^6 is (1/64), so (1/6)(1/64) = 1/(384)
2. (-1/2)^5: (-1/32), so the term is (-1/32)
3. (5/2)(-1/2)^4: (-1/2)^4 is 1/16, so (5/2)(1/16) = 5/32
4. (8/3)(-1/2)^3: (-1/2)^3 is -1/8, so (8/3)(-1/8) = -1/24
5. (1/2)(-1/2)^2: (1/2)(1/4) = 1/8

Adding these up:

1/384 - 1/32 + 5/32 - 1/24 + 1/8

Let me convert all to 384 denominator for easier addition:

1/384 - 12/384 + 60/384 - 16/384 + 48/384

Adding numerators: 1 -12 +60 -16 +48 = (1 -12) = -11; (-11 +60)=49; (49 -16)=33; (33 +48)=81. So total is 81/384. Simplify that: divide numerator and denominator by 3: 27/128. Wait, 81 ÷3=27, 384 ÷3=128. So 27/128 ≈ 0.2109375.

Wait, let me check that again. Wait, 81/384: 81 divided by 3 is 27, 384 divided by 3 is 128. Yes, 27/128. Correct.

Now compute F(-3/2):

Each term at x = -3/2:

1. (1/6)(-3/2)^6: (-3/2)^6 is (729/64), so (1/6)(729/64) = 729/(6*64) = 729/384 = 243/128 ≈ 1.8984375

2. (-3/2)^5: (-243/32), so the term is (-243/32)

3. (5/2)(-3/2)^4: (-3/2)^4 is 81/16, so (5/2)(81/16) = 405/32 ≈12.65625

4. (8/3)(-3/2)^3: (-3/2)^3 is -27/8, so (8/3)(-27/8) = (8/3)*(27/8) = 27/3 = 9

5. (1/2)(-3/2)^2: (-3/2)^2 is 9/4, so (1/2)(9/4) = 9/8 ≈1.125

Now sum all these terms:

243/128 -243/32 +405/32 +9 +9/8

Let me convert all terms to 128 denominator:

243/128 - (243/32)*(4/4) = -243*4/128 = -972/128

405/32 = 405*4/128 = 1620/128

9 = 1152/128

9/8 = 144/128

So adding all terms:

243/128 -972/128 +1620/128 +1152/128 +144/128

Sum numerators: 243 -972 +1620 +1152 +144

Let's compute step by step:

243 -972 = -729

-729 +1620 = 891

891 +1152 = 2043

2043 +144 = 2187

So 2187/128 ≈17.0859375

Therefore, F(-3/2) = 2187/128

Now, the definite integral is F(-1/2) - F(-3/2) = (27/128) - (2187/128) = (27 -2187)/128 = (-2160)/128

Simplify this fraction:

Divide numerator and denominator by 16: -2160 ÷16 = -135; 128 ÷16=8. So -135/8.

Wait, 2160 ÷16: 16*135=2160, yes. So -135/8. Which is -16.875.

Wait, but let me check again. 27 -2187 is indeed -2160. Then -2160/128. Let's divide numerator and denominator by 8: -270/16. Then divide by 2: -135/8. Yes, that's correct. So the exact value is -135/8.

But wait, let me check the calculations again because sometimes when dealing with negative signs, mistakes can happen. Let me verify each step.

First, F(-1/2):

(1/6)(-1/2)^6: (-1/2)^6 is positive 1/64, so 1/(6*64)=1/384 ≈0.0026041667

Then, the second term: (-1/2)^5 is -1/32, so that term is -1/32 ≈-0.03125

Third term: (5/2)(-1/2)^4. (-1/2)^4 is 1/16, so 5/2 *1/16=5/32≈0.15625

Fourth term: (8/3)(-1/2)^3. (-1/2)^3 is -1/8, so 8/3*(-1/8)= -1/3 ≈-0.3333333333

Fifth term: (1/2)(-1/2)^2. (-1/2)^2 is 1/4, so 1/2*1/4=1/8=0.125

Adding all these:

0.0026041667 -0.03125 +0.15625 -0.3333333333 +0.125

Let me compute step by step:

Start with 0.0026041667 -0.03125 = -0.0286458333

Then -0.0286458333 +0.15625 = 0.1276041667

0.1276041667 -0.3333333333 = -0.2057291666

-0.2057291666 +0.125 = -0.0807291666

Wait, but earlier I had 27/128 which is approximately 0.2109375. Wait, this is conflicting. There's a mistake here. Wait, wait, I must have messed up the conversion to 384 denominator.

Wait, let's recalculate F(-1/2) properly. Let me redo the calculation step by step.

F(-1/2) = (1/6)(-1/2)^6 + (-1/2)^5 + (5/2)(-1/2)^4 + (8/3)(-1/2)^3 + (1/2)(-1/2)^2

Compute each term:

1. (1/6)(-1/2)^6: (-1/2)^6 = 1/64, so (1/6)(1/64) = 1/384 ≈0.0026041667

2. (-1/2)^5: (-1/32) ≈-0.03125

3. (5/2)(-1/2)^4: (-1/2)^4 =1/16, so (5/2)(1/16)=5/32≈0.15625

4. (8/3)(-1/2)^3: (-1/2)^3= -1/8, so (8/3)(-1/8)= -1/3 ≈-0.3333333333

5. (1/2)(-1/2)^2: (1/2)(1/4)=1/8=0.125

Now sum all terms:

0.0026041667 -0.03125 +0.15625 -0.3333333333 +0.125

Let's compute step by step:

Start with 0.0026041667 -0.03125 = -0.0286458333

Then add 0.15625: -0.0286458333 +0.15625 = 0.1276041667

Subtract 0.3333333333: 0.1276041667 -0.3333333333 = -0.2057291666

Add 0.125: -0.2057291666 +0.125 = -0.0807291666

Wait, that's approximately -0.0807291666, which is -0.0807291666. But earlier, when I converted to 384 denominator, I got 81/384 = 27/128 ≈0.2109375. That's a discrepancy. So there's a mistake in my initial calculation. Hmm, where did I go wrong?

Wait, when I converted each term to 384 denominator:

Original terms:

1/384 -1/32 +5/32 -1/24 +1/8

Convert each fraction to denominator 384:

1/384 remains 1/384

-1/32 = -12/384

5/32 = 60/384

-1/24 = -16/384 (since 1/24 = 16/384? Wait, 384 ÷24=16, so 1/24 = 16/384. So -1/24 is -16/384.

1/8 = 48/384

So sum: 1 -12 +60 -16 +48 = 81. So 81/384 = 27/128 ≈0.2109375. But when I calculated numerically, I got -0.0807... That's a problem. So which one is correct?

Wait, there's a mistake here. Let me check the antiderivative again. Wait, the antiderivative is:

F(x) = (1/6)x⁶ + x⁵ + (5/2)x⁴ + (8/3)x³ + (1/2)x² + C

But when evaluating at x = -1/2, each term is:

1. (1/6)(-1/2)^6: correct as 1/384

2. x⁵: (-1/2)^5 = -1/32

3. (5/2)x⁴: (5/2)(1/16) = 5/32

4. (8/3)x³: (8/3)(-1/8) = -1/3

5. (1/2)x²: (1/2)(1/4) = 1/8

So the terms are correct. Then when adding:

1/384 -1/32 +5/32 -1/3 +1/8

Wait, but in my initial conversion to 384 denominator, I had -1/24 instead of -1/3. Oh! There's the mistake. The fourth term is (8/3)x³ evaluated at x=-1/2 gives (8/3)*(-1/8) = -1/3, not -1/24. So in the initial step, I incorrectly converted -1/3 to -16/384, but that's wrong. Because 1/3 is 128/384, so -1/3 is -128/384. So the correct conversion is:

1/384 (from first term)

-1/32 = -12/384

+5/32 = +60/384

-1/3 = -128/384

+1/8 = +48/384

Now sum numerators: 1 -12 +60 -128 +48 = (1 -12) = -11; (-11 +60)=49; (49 -128)= -79; (-79 +48)= -31. So total is -31/384 ≈-0.0807291666

But earlier, when I thought it was 81/384, I was wrong because I used -1/24 instead of -1/3. So the correct value for F(-1/2) is -31/384 ≈-0.0807291666

Similarly, I must have made a mistake in calculating F(-3/2). Let's redo that.

F(-3/2) = (1/6)(-3/2)^6 + (-3/2)^5 + (5/2)(-3/2)^4 + (8/3)(-3/2)^3 + (1/2)(-3/2)^2

Compute each term:

1. (1/6)(-3/2)^6: (-3/2)^6 = (729/64), so (1/6)(729/64) = 729/384 = 243/128 ≈1.8984375

2. (-3/2)^5 = -243/32 ≈-7.59375

3. (5/2)(-3/2)^4: (-3/2)^4 =81/16, so (5/2)(81/16)=405/32 ≈12.65625

4. (8/3)(-3/2)^3: (-3/2)^3 = -27/8, so (8/3)(-27/8) = -9

5. (1/2)(-3/2)^2: (-3/2)^2=9/4, so (1/2)(9/4)=9/8 ≈1.125

Now sum all terms:

243/128 -243/32 +405/32 -9 +9/8

Let's convert all terms to 128 denominator:

243/128

-243/32 = -243*4/128 = -972/128

405/32 = 405*4/128 = 1620/128

-9 = -1152/128

9/8 = 144/128

Now sum numerators:

243 -972 +1620 -1152 +144

Compute step by step:

243 -972 = -729

-729 +1620 = 891

891 -1152 = -261

-261 +144 = -117

So total is -117/128 ≈-0.9140625

Wait, but earlier I had 2187/128 ≈17.0859375. That was a mistake. So where did I go wrong before?

Ah, I see. In the previous calculation, I think I messed up the sign for the fourth term. Let me check:

The fourth term is (8/3)x³ evaluated at x=-3/2. So (8/3)*(-3/2)^3. (-3/2)^3 is -27/8. So (8/3)*(-27/8) = -27/3 = -9. So that term is -9. But in my initial calculation, I had written it as +9. That's the mistake. So the fourth term is -9, not +9. Therefore, in the previous calculation, I incorrectly added +9 instead of -9, leading to an incorrect positive value. So the correct sum is:

243/128 -243/32 +405/32 -9 +9/8

Which converts to:

243/128 -972/128 +1620/128 -1152/128 +144/128

Summing numerators: 243 -972 +1620 -1152 +144

As before, which gives -117/128 ≈-0.9140625

Therefore, F(-3/2) = -117/128 ≈-0.9140625

Therefore, the definite integral is F(-1/2) - F(-3/2) = (-31/384) - (-117/128) = (-31/384) + (117/128)

Convert 117/128 to 384 denominator: 117/128 = (117*3)/(128*3) = 351/384

So, -31/384 +351/384 = (351 -31)/384 = 320/384 = 320 ÷ 64 =5, 384 ÷64=6. So 5/6 ≈0.8333333333

Wait, 320/384 simplifies by dividing numerator and denominator by 32: 10/12, which is 5/6. So the exact value is 5/6 ≈0.8333333333.

But wait, this contradicts the previous result. So where was the mistake?

Wait, let's recheck:

F(-1/2) = -31/384 ≈-0.0807291666

F(-3/2) = -117/128 ≈-0.9140625

So F(-1/2) - F(-3/2) = (-0.0807291666) - (-0.9140625) = (-0.0807291666) +0.9140625 = 0.8333333334

Which is approximately 5/6 ≈0.8333333333. So the exact value is 5/6.

Wait, how did we get 320/384? 320 divided by 64 is 5, 384 divided by 64 is 6. So 5/6. Yes.

So the integral from -3/2 to -1/2 is 5/6. So the exact answer is 5/6, and numerically approximately 0.8333333333.

But wait, this contradicts the initial calculation where I thought the answer was -135/8. Clearly, I made a mistake in the initial steps by miscalculating the signs and terms, especially in the fourth term of F(-1/2) and F(-3/2). So the correct answer is 5/6.

Let me verify this with another approach. Maybe expanding the polynomial and integrating term by term.

Alternatively, perhaps there's a smarter way. Let me check if the integrand can be factored or simplified.

The integrand is x⁵ +5x⁴ +10x³ +8x² +x.

Hmm, maybe try to factor it. Let's see:

Let me try to factor the polynomial. Let's check for rational roots using Rational Root Theorem. Possible roots are ±1. Let's test x=-1:

(-1)^5 +5(-1)^4 +10(-1)^3 +8(-1)^2 +(-1) = -1 +5(1) +10(-1) +8(1) -1 = -1 +5 -10 +8 -1 = ( -1 +5)=4; (4 -10)= -6; (-6 +8)=2; (2 -1)=1 ≠0. So x=-1 is not a root.

Try x=0: 0 +0 +0 +0 +0=0. So x=0 is a root. So we can factor out x:

x(x⁴ +5x³ +10x² +8x +1)

Now, let's factor the quartic polynomial x⁴ +5x³ +10x² +8x +1.

Try to factor this quartic. Let's try to factor it into quadratics: (x² + ax + b)(x² + cx + d) = x⁴ + (a + c)x³ + (ac + b + d)x² + (ad + bc)x + bd.

Set coefficients equal:

1. a + c =5

2. ac + b + d =10

3. ad + bc =8

4. bd=1

Since bd=1, possible pairs (b=1, d=1) or (b=-1, d=-1). Let's try b=1, d=1.

Then equation 3: a*1 + c*1 = a +c =5, which matches equation 1. But equation 2: ac +1 +1=ac +2=10 ⇒ ac=8.

So from equation 1: a +c=5, and ac=8. So solving quadratic equation t² -5t +8=0. Discriminant: 25 -32= -7 <0. No real solutions. So that doesn't work.

Try b=-1, d=-1. Then equation 3: a*(-1) +c*(-1)= -a -c=8. But from equation 1, a +c=5. So -5=8? No. Contradiction. So this doesn't work.

Alternative approach: Maybe the quartic can be factored as (x³ + ...)(x + ...). Let's try to find a root. Let's check x=-1 again for the quartic:

(-1)^4 +5(-1)^3 +10(-1)^2 +8(-1) +1 =1 -5 +10 -8 +1= (1-5)= -4; (-4+10)=6; (6-8)= -2; (-2+1)= -1 ≠0. Not a root.

x= -0.5: (0.0625) +5*(-0.125) +10*(0.25) +8*(-0.5) +1 =0.0625 -0.625 +2.5 -4 +1= (0.0625 -0.625)= -0.5625; (-0.5625 +2.5)=1.9375; (1.9375 -4)= -2.0625; (-2.0625 +1)= -1.0625 ≠0.

Not a root. Maybe x= -2:

x⁴=16, 5x³=5*(-8)= -40, 10x²=10*4=40, 8x=8*(-2)= -16, +1. So 16 -40 +40 -16 +1=1. Not zero.

Hmm, perhaps this polynomial doesn't factor nicely. So maybe integrating term by term is the way to go, which we did earlier.

But according to the corrected calculation, the integral is 5/6. Let me check with numerical approximation.

Compute the integral numerically using approximate values.

The integrand is x⁵ +5x⁴ +10x³ +8x² +x. Let's compute the integral from -1.5 to -0.5.

We can approximate it numerically. Let's use a numerical method like Simpson's rule for better accuracy, but since it's a polynomial, Simpson's rule should be exact for polynomials up to degree 3. However, our integrand is degree 5, so Simpson's rule with sufficient intervals would give an accurate result. Alternatively, since we already have the exact answer as 5/6 ≈0.8333333333, let's check with a simple approximation.

Alternatively, compute the definite integral using the exact antiderivative:

F(x) = (1/6)x⁶ +x⁵ + (5/2)x⁴ + (8/3)x³ + (1/2)x²

Evaluate at x=-0.5:

(1/6)(-0.5)^6 + (-0.5)^5 + (5/2)(-0.5)^4 + (8/3)(-0.5)^3 + (1/2)(-0.5)^2

Compute each term:

(1/6)(1/64) = 1/384 ≈0.0026041667

(-1/32) ≈-0.03125

(5/2)(1/16)=5/32≈0.15625

(8/3)(-1/8)= -1/3 ≈-0.3333333333

(1/2)(1/4)=1/8=0.125

Sum: 0.0026041667 -0.03125 +0.15625 -0.3333333333 +0.125 ≈-0.0807291666

At x=-1.5:

(1/6)(-1.5)^6 + (-1.5)^5 + (5/2)(-1.5)^4 + (8/3)(-1.5)^3 + (1/2)(-1.5)^2

Compute each term:

(-1.5)^6 = (3/2)^6 = 729/64 ≈11.390625

(1/6)*11.390625 ≈1.8984375

(-1.5)^5 = -7.59375

(5/2)*(5.0625) = (5/2)*(81/16) = 405/32 ≈12.65625

(8/3)*(-3.375) = (8/3)*(-27/8) = -9

(1/2)*(2.25) =1.125

Sum: 1.8984375 -7.59375 +12.65625 -9 +1.125 ≈(1.8984375 -7.59375)= -5.6953125; (-5.6953125 +12.65625)=6.9609375; (6.9609375 -9)= -2.0390625; (-2.0390625 +1.125)= -0.9140625

So F(-1.5) ≈-0.9140625

Therefore, F(-0.5) - F(-1.5) ≈ (-0.0807291666) - (-0.9140625) = 0.8333333334, which is approximately 5/6 ≈0.8333333333. So the exact answer is 5/6.

Therefore, the definite integral is 5/6, and the numerical approximation is approximately 0.8333333333.

But wait, earlier when I thought the answer was -135/8, that was due to incorrect sign handling. The correct answer is 5/6. So the final answer should be {"answer": "\dfrac{5}{6}", "numerical_answer": 0.8333333333}
</think>

{"answer": "\\dfrac{5}{6}", "numerical_answer": 0.8333333333}