
To calculate the definite integral \(\int_{0}^{1} \arcsin(x) \arccos(x) \, dx\), we start by using the identity \(\arcsin(x) + \arccos(x) = \frac{\pi}{2}\) for \(x \in [-1, 1]\). Let \(A = \arcsin(x)\), so \(\arccos(x) = \frac{\pi}{2} - A\). The integrand becomes:

\[
\arcsin(x) \arccos(x) = A \left( \frac{\pi}{2} - A \right) = \frac{\pi}{2} A - A^2
\]

Thus, the integral splits into two parts:

\[
\int_{0}^{1} \arcsin(x) \arccos(x) \, dx = \frac{\pi}{2} \int_{0}^{1} \arcsin(x) \, dx - \int_{0}^{1} (\arcsin(x))^2 \, dx
\]

### Step 1: Compute \(\int_{0}^{1} \arcsin(x) \, dx\)
Using integration by parts with \(u = \arcsin(x)\) and \(dv = dx\), we get \(du = \frac{1}{\sqrt{1 - x^2}} \, dx\) and \(v = x\). The integral becomes:

\[
\int \arcsin(x) \, dx = x \arcsin(x) - \int \frac{x}{\sqrt{1 - x^2}} \, dx
\]

For the remaining integral, substitute \(t = 1 - x^2\), \(dt = -2x \, dx\), so:

\[
\int \frac{x}{\sqrt{1 - x^2}} \, dx = -\sqrt{1 - x^2} + C
\]

Thus,

\[
\int \arcsin(x) \, dx = x \arcsin(x) + \sqrt{1 - x^2} + C
\]

Evaluating from \(0\) to \(1\):

\[
\left[ x \arcsin(x) + \sqrt{1 - x^2} \right]_{0}^{1} = \left( 1 \cdot \frac{\pi}{2} + 0 \right) - \left( 0 + 1 \right) = \frac{\pi}{2} - 1
\]

### Step 2: Compute \(\int_{0}^{1} (\arcsin(x))^2 \, dx\)
Again, use integration by parts with \(u = (\arcsin(x))^2\) and \(dv = dx\), so \(du = \frac{2 \arcsin(x)}{\sqrt{1 - x^2}} \, dx\) and \(v = x\). The integral becomes:

\[
\int (\arcsin(x))^2 \, dx = x (\arcsin(x))^2 - 2 \int \frac{x \arcsin(x)}{\sqrt{1 - x^2}} \, dx
\]

For the remaining integral, substitute \(t = \arcsin(x)\) (so \(x = \sin(t)\), \(dx = \cos(t) \, dt\), and \(\sqrt{1 - x^2} = \cos(t)\)):

\[
\int \frac{x \arcsin(x)}{\sqrt{1 - x^2}} \, dx = \int t \sin(t) \, dt
\]

Using integration by parts again (\(u = t\), \(dv = \sin(t) \, dt\)):

\[
\int t \sin(t) \, dt = -t \cos(t) + \sin(t) + C
\]

Substituting back \(t = \arcsin(x)\), \(\cos(t) = \sqrt{1 - x^2}\), and \(\sin(t) = x\):

\[
\int \frac{x \arcsin(x)}{\sqrt{1 - x^2}} \, dx = -\arcsin(x) \sqrt{1 - x^2} + x + C
\]

Thus,

\[
\int (\arcsin(x))^2 \, dx = x (\arcsin(x))^2 + 2 \arcsin(x) \sqrt{1 - x^2} - 2x + C
\]

Evaluating from \(0\) to \(1\):

\[
\left[ x (\arcsin(x))^2 + 2 \arcsin(x) \sqrt{1 - x^2} - 2x \right]_{0}^{1} = \left( 1 \cdot \left( \frac{\pi}{2} \right)^2 + 0 - 2 \cdot 1 \right) - 0 = \frac{\pi^2}{4} - 2
\]

### Step 3: Combine the results
The original integral is:

\[
\frac{\pi}{2} \left( \frac{\pi}{2} - 1 \right) - \left( \frac{\pi^2}{4} - 2 \right) = \frac{\pi^2}{4} - \frac{\pi}{2} - \frac{\pi^2}{4} + 2 = 2 - \frac{\pi}{2}
\]

### Numerical Approximation
Using \(\pi \approx 3.141592653589793\), we get:

\[
2 - \frac{\pi}{2} \approx 2 - 1.5707963267948966 = 0.4292036732051034
\]

Rounded to 10 decimal places, this is \(0.4292036732\).

{"answer": "2 - \\frac{\\pi}{2}", "numerical_answer": "0.4292036732"}