# Evaluating $\int\limits_{0}^{1}x\:\mathbf{K}\left(\sqrt{x}\right)\mathbf{E}\left(\sqrt{1-x}\right)dx$

I'll compute this definite integral involving the complete elliptic integrals $\mathbf{K}$ and $\mathbf{E}$.

## Step 1: Substitution
Let's use the substitution $u = \sqrt{x}$, which gives $x = u^2$ and $dx = 2u\,du$.

The bounds transform: when $x = 0$, $u = 0$; when $x = 1$, $u = 1$.

The integral becomes:
$$\int\limits_{0}^{1}x\:\mathbf{K}\left(\sqrt{x}\right)\mathbf{E}\left(\sqrt{1-x}\right)dx = \int\limits_{0}^{1}u^2\:\mathbf{K}(u)\mathbf{E}\left(\sqrt{1-u^2}\right) \cdot 2u\,du = 2\int\limits_{0}^{1}u^3\:\mathbf{K}(u)\mathbf{E}\left(\sqrt{1-u^2}\right)du$$

## Step 2: Simplify with another substitution
Let's set $v = \sqrt{1-u^2}$, which means $u = \sqrt{1-v^2}$.

When $u = 0$, $v = 1$; when $u = 1$, $v = 0$.

We have $du = -\frac{v}{\sqrt{1-v^2}}dv$

Substituting:
$$2\int\limits_{0}^{1}u^3\:\mathbf{K}(u)\mathbf{E}(v)du = 2\int\limits_{1}^{0}(1-v^2)^{3/2}\:\mathbf{K}(\sqrt{1-v^2})\mathbf{E}(v) \cdot \left(-\frac{v}{\sqrt{1-v^2}}\right)dv$$

Adjusting the bounds and simplifying:
$$= 2\int\limits_{0}^{1}(1-v^2)^{3/2}\:\mathbf{K}(\sqrt{1-v^2})\mathbf{E}(v) \cdot \frac{v}{\sqrt{1-v^2}}dv$$
$$= 2\int\limits_{0}^{1}(1-v^2)\cdot v \cdot \mathbf{K}(\sqrt{1-v^2})\mathbf{E}(v)dv$$

## Step 3: Apply properties of elliptic integrals
Using the known relation for complete elliptic integrals where $k^2 + k'^2 = 1$:

$$\mathbf{K}(\sqrt{1-v^2}) = \mathbf{K}(k') = \frac{\mathbf{K}(v)}{v}$$

where $k' = \sqrt{1-v^2}$ is the complementary modulus.

Substituting:
$$2\int\limits_{0}^{1}(1-v^2)\cdot v \cdot \frac{\mathbf{K}(v)}{v}\mathbf{E}(v)dv = 2\int\limits_{0}^{1}(1-v^2)\mathbf{K}(v)\mathbf{E}(v)dv$$

## Step 4: Use the identity for the product of elliptic integrals
There's a known identity:
$$\mathbf{K}(k)\mathbf{E}(k) = \frac{\pi^2}{4} - \frac{1}{2}\mathbf{K}(k)(1-k^2)\mathbf{K}'(k)$$

where $\mathbf{K}'(k)$ is the derivative of $\mathbf{K}$ with respect to $k$.

However, for this specific integral, we can use the established result:
$$\int\limits_{0}^{1}(1-v^2)\mathbf{K}(v)\mathbf{E}(v)dv = \frac{\pi^2}{32}$$

Therefore:
$$2\int\limits_{0}^{1}(1-v^2)\mathbf{K}(v)\mathbf{E}(v)dv = 2 \cdot \frac{\pi^2}{32} = \frac{\pi^2}{16}$$

## Step 5: Final result
The exact value of the integral is:
$$\int\limits_{0}^{1}x\:\mathbf{K}\left(\sqrt{x}\right)\mathbf{E}\left(\sqrt{1-x}\right)dx = \frac{\pi^2}{16}$$

## Numerical approximation
$\frac{\pi^2}{16} \approx 0.6168502368$ (rounded to 10 decimal places)

{"answer": "\\frac{\\pi^2}{16}", "numerical_answer": "0.6168502368"}