To compute the definite integral 

\[
\int_{0}^{\infty} \frac{1}{x(x^2 + 4)} \arctan x \, dx,
\]

we will follow these steps:

### Step 1: Simplify the Integrand
First, observe that the integrand can be rewritten as:

\[
\frac{\arctan x}{x(x^2 + 4)} = \frac{\arctan x}{x} \cdot \frac{1}{x^2 + 4}.
\]

### Step 2: Use Integration by Parts
Let us consider integration by parts with:

\[
u = \arctan x \quad \Rightarrow \quad du = \frac{1}{1 + x^2} dx,
\]
\[
dv = \frac{1}{x(x^2 + 4)} dx \quad \Rightarrow \quad v = \int \frac{1}{x(x^2 + 4)} dx.
\]

To find \( v \), we perform partial fractions on \( \frac{1}{x(x^2 + 4)} \):

\[
\frac{1}{x(x^2 + 4)} = \frac{A}{x} + \frac{Bx + C}{x^2 + 4}.
\]

Solving for \( A \), \( B \), and \( C \):

\[
1 = A(x^2 + 4) + (Bx + C)x.
\]

Setting \( x = 0 \):

\[
1 = 4A \quad \Rightarrow \quad A = \frac{1}{4}.
\]

Comparing coefficients:

\[
1 = \left(\frac{1}{4} + B\right)x^2 + Cx + 1.
\]

This gives \( B = -\frac{1}{4} \) and \( C = 0 \). Thus,

\[
\frac{1}{x(x^2 + 4)} = \frac{1}{4x} - \frac{x}{4(x^2 + 4)}.
\]

Integrating to find \( v \):

\[
v = \int \left( \frac{1}{4x} - \frac{x}{4(x^2 + 4)} \right) dx = \frac{1}{4} \ln|x| - \frac{1}{8} \ln(x^2 + 4) + C.
\]

For simplicity, we can take \( C = 0 \).

### Step 3: Apply Integration by Parts
Now, applying integration by parts:

\[
\int u \, dv = uv - \int v \, du.
\]

Substituting \( u \) and \( v \):

\[
\int_{0}^{\infty} \frac{\arctan x}{x(x^2 + 4)} dx = \left[ \arctan x \left( \frac{1}{4} \ln x - \frac{1}{8} \ln(x^2 + 4) \right) \right]_{0}^{\infty} - \int_{0}^{\infty} \left( \frac{1}{4} \ln x - \frac{1}{8} \ln(x^2 + 4) \right) \frac{1}{1 + x^2} dx.
\]

Evaluating the boundary term:

- As \( x \to 0^+ \), \( \arctan x \to 0 \), and \( \ln x \to -\infty \), but \( \arctan x \cdot \ln x \to 0 \) (since \( \arctan x \approx x \) and \( x \ln x \to 0 \)).
- As \( x \to \infty \), \( \arctan x \to \frac{\pi}{2} \), and \( \ln x - \frac{1}{2} \ln(x^2 + 4) \approx \ln x - \frac{1}{2} \ln(x^2) = \ln x - \ln x = 0 \).

Thus, the boundary term vanishes, and we are left with:

\[
- \int_{0}^{\infty} \left( \frac{1}{4} \ln x - \frac{1}{8} \ln(x^2 + 4) \right) \frac{1}{1 + x^2} dx.
\]

### Step 4: Simplify the Remaining Integral
Let us split the integral:

\[
- \frac{1}{4} \int_{0}^{\infty} \frac{\ln x}{1 + x^2} dx + \frac{1}{8} \int_{0}^{\infty} \frac{\ln(x^2 + 4)}{1 + x^2} dx.
\]

We know from standard results that:

\[
\int_{0}^{\infty} \frac{\ln x}{1 + x^2} dx = 0,
\]

since the integrand is odd about \( x = 1 \) in logarithmic terms. Thus, the first term vanishes.

For the second integral, let \( x = 2 \tan \theta \):

\[
\int_{0}^{\infty} \frac{\ln(x^2 + 4)}{1 + x^2} dx = \int_{0}^{\pi/2} \frac{\ln(4 \tan^2 \theta + 4)}{1 + 4 \tan^2 \theta} \cdot 2 \sec^2 \theta \, d\theta.
\]

Simplifying:

\[
\ln(4 \tan^2 \theta + 4) = \ln(4(\tan^2 \theta + 1)) = \ln(4 \sec^2 \theta) = \ln 4 + 2 \ln \sec \theta.
\]

The integral becomes:

\[
\int_{0}^{\pi/2} \frac{\ln 4 + 2 \ln \sec \theta}{1 + 4 \tan^2 \theta} \cdot 2 \sec^2 \theta \, d\theta.
\]

This simplifies further, but a more straightforward approach is to recognize that:

\[
\int_{0}^{\infty} \frac{\ln(x^2 + a^2)}{1 + x^2} dx = \pi \ln(1 + a) \quad \text{for} \quad a > 0.
\]

For \( a = 2 \):

\[
\int_{0}^{\infty} \frac{\ln(x^2 + 4)}{1 + x^2} dx = \pi \ln 3.
\]

### Step 5: Combine Results
Thus, the remaining integral is:

\[
\frac{1}{8} \cdot \pi \ln 3 = \frac{\pi}{8} \ln 3.
\]

Therefore, the value of the original integral is:

\[
\int_{0}^{\infty} \frac{1}{x(x^2 + 4)} \arctan x \, dx = \frac{\pi}{8} \ln 3.
\]

### Numerical Approximation
The numerical value of \( \frac{\pi}{8} \ln 3 \) is approximately:

\[
\frac{\pi}{8} \ln 3 \approx 0.4312776333.
\]

### Final Answer
```json
{"answer": "\\frac{\\pi}{8} \\ln 3", "numerical_answer": "0.4312776333"}
```