# Evaluating $\int\limits_{0}^{2}H_{3}\left(\sqrt{x(2-x)}\right)dx$

First, let me recall that $H_3(x)$ is the 3rd Hermite polynomial, which is:

$$H_3(x) = 8x^3 - 12x$$

## Step 1: Substitute the expression into the Hermite polynomial

Let $u = \sqrt{x(2-x)}$. Then:

$$H_3(u) = 8u^3 - 12u = 8(\sqrt{x(2-x)})^3 - 12\sqrt{x(2-x)}$$

So our integral becomes:
$$\int\limits_{0}^{2}[8(\sqrt{x(2-x)})^3 - 12\sqrt{x(2-x)}]dx$$

## Step 2: Analyze the integrand

Let's examine the geometry of the expression $\sqrt{x(2-x)}$. This can be rewritten as:
$$\sqrt{x(2-x)} = \sqrt{2x - x^2} = \sqrt{1-(x-1)^2}$$

This represents a semicircle with radius 1 centered at $(1,0)$. 

## Step 3: Use substitution

Let $x = 1 + \sin\theta$, which gives $dx = \cos\theta\,d\theta$

When $x = 0$, we have $1 + \sin\theta = 0$, so $\sin\theta = -1$, which gives $\theta = -\frac{\pi}{2}$
When $x = 2$, we have $1 + \sin\theta = 2$, so $\sin\theta = 1$, which gives $\theta = \frac{\pi}{2}$

With this substitution:
$$\sqrt{x(2-x)} = \sqrt{(1+\sin\theta)(1-\sin\theta)} = \sqrt{1-\sin^2\theta} = \cos\theta$$

So our integral becomes:
$$\int_{-\pi/2}^{\pi/2}[8\cos^3\theta - 12\cos\theta]\cos\theta\,d\theta = \int_{-\pi/2}^{\pi/2}[8\cos^4\theta - 12\cos^2\theta]\,d\theta$$

## Step 4: Evaluate the integral

For the first term:
$$\int\cos^4\theta\,d\theta = \int\left(\frac{3+4\cos(2\theta)+\cos(4\theta)}{8}\right)\,d\theta = \frac{3\theta}{8} + \frac{\sin(2\theta)}{4} + \frac{\sin(4\theta)}{32}$$

For the second term:
$$\int\cos^2\theta\,d\theta = \int\left(\frac{1+\cos(2\theta)}{2}\right)\,d\theta = \frac{\theta}{2} + \frac{\sin(2\theta)}{4}$$

Evaluating from $-\pi/2$ to $\pi/2$:

For $8\cos^4\theta$:
$$8\left[\frac{3\theta}{8} + \frac{\sin(2\theta)}{4} + \frac{\sin(4\theta)}{32}\right]_{-\pi/2}^{\pi/2} = 8\left[\frac{3\pi/2}{8} - \frac{3(-\pi/2)}{8}\right] = 8 \cdot \frac{3\pi}{8} = 3\pi$$

Since $\sin(2\theta)$ and $\sin(4\theta)$ are odd functions, their contributions from $-\pi/2$ to $\pi/2$ cancel out.

For $-12\cos^2\theta$:
$$-12\left[\frac{\theta}{2} + \frac{\sin(2\theta)}{4}\right]_{-\pi/2}^{\pi/2} = -12\left[\frac{\pi/2}{2} - \frac{-\pi/2}{2}\right] = -12 \cdot \frac{\pi}{2} = -6\pi$$

Again, the $\sin(2\theta)$ term cancels out due to symmetry.

## Step 5: Calculate the final result

$$\int\limits_{0}^{2}H_{3}\left(\sqrt{x(2-x)}\right)dx = 3\pi - 6\pi = -3\pi$$

## Numerical approximation

$$-3\pi \approx -9.4247779607$$

{"answer": "-3\\pi", "numerical_answer": "-9.4247779607"}