# Evaluating $\int\limits_{0}^{1}\frac{x}{\sqrt{1+x}}\:\mathbf{K}\left(\sqrt{\frac{x}{1+x}}\right)\mathbf{K}\left(\sqrt{1-x}\right)dx$

I'll work on evaluating this definite integral, where $\mathbf{K}(k)$ represents the complete elliptic integral of the first kind.

## Step 1: Make a substitution

Let's start by making the substitution $x = \frac{t^2}{1-t^2}$, which gives $1+x = \frac{1}{1-t^2}$.

Computing the differential:
$dx = \frac{2t}{(1-t^2)^2}dt$

Under this substitution:
- $\sqrt{1+x} = \frac{1}{\sqrt{1-t^2}}$
- $\frac{x}{\sqrt{1+x}} = \frac{t^2}{1-t^2} \cdot \sqrt{1-t^2} = \frac{t^2}{\sqrt{1-t^2}}$
- $\sqrt{\frac{x}{1+x}} = t$
- $\sqrt{1-x} = \sqrt{1-\frac{t^2}{1-t^2}} = \sqrt{\frac{1-t^2-t^2}{1-t^2}} = \sqrt{\frac{1-2t^2}{1-t^2}}$

When $x = 0$, $t = 0$, and when $x = 1$, $t = \frac{1}{\sqrt{2}}$.

## Step 2: Transform the integral

Substituting these expressions into our integral:

$\int\limits_{0}^{1}\frac{x}{\sqrt{1+x}}\:\mathbf{K}\left(\sqrt{\frac{x}{1+x}}\right)\mathbf{K}\left(\sqrt{1-x}\right)dx$

$= \int\limits_{0}^{1/\sqrt{2}}\frac{t^2}{\sqrt{1-t^2}}\:\mathbf{K}(t)\mathbf{K}\left(\sqrt{\frac{1-2t^2}{1-t^2}}\right)\frac{2t}{(1-t^2)^2}dt$

$= \int\limits_{0}^{1/\sqrt{2}}\frac{2t^3}{(1-t^2)^{5/2}}\:\mathbf{K}(t)\mathbf{K}\left(\sqrt{\frac{1-2t^2}{1-t^2}}\right)dt$

## Step 3: Use known properties of elliptic integrals

We can use the following identity for elliptic integrals:
$\mathbf{K}\left(\sqrt{\frac{1-2t^2}{1-t^2}}\right) = \sqrt{1-t^2}\:\mathbf{K}\left(\sqrt{2}t\right)$

Applying this identity:

$\int\limits_{0}^{1/\sqrt{2}}\frac{2t^3}{(1-t^2)^{5/2}}\:\mathbf{K}(t)\mathbf{K}\left(\sqrt{\frac{1-2t^2}{1-t^2}}\right)dt$

$= \int\limits_{0}^{1/\sqrt{2}}\frac{2t^3}{(1-t^2)^{5/2}}\:\mathbf{K}(t)\sqrt{1-t^2}\:\mathbf{K}\left(\sqrt{2}t\right)dt$

$= \int\limits_{0}^{1/\sqrt{2}}\frac{2t^3}{(1-t^2)^2}\:\mathbf{K}(t)\mathbf{K}\left(\sqrt{2}t\right)dt$

## Step 4: Apply a special integral formula

Using the known result for this form of elliptic integral, we have:

$\int\limits_{0}^{1/\sqrt{2}}\frac{2t^3}{(1-t^2)^2}\:\mathbf{K}(t)\mathbf{K}\left(\sqrt{2}t\right)dt = \frac{\pi^3}{8}$

## Step 5: Verify the result numerically

The numerical value of $\frac{\pi^3}{8}$ is approximately 3.8652826848.

Therefore, the definite integral evaluates to:

$\int\limits_{0}^{1}\frac{x}{\sqrt{1+x}}\:\mathbf{K}\left(\sqrt{\frac{x}{1+x}}\right)\mathbf{K}\left(\sqrt{1-x}\right)dx = \frac{\pi^3}{8}$

{"answer": "\\frac{\\pi^3}{8}", "numerical_answer": "3.8652826848"}