Let's evaluate the definite integral:
\[
I = \int_0^{2} x^{1/2} (2-x)^{-1/2} \cos\left( \sqrt{x(2-x)} \right)\; dx
\]

### Step 1: Substitution

Let \( x = 2 \sin^2\theta \), so as \( x \) goes from \( 0 \) to \( 2 \):
- When \( x = 0 \): \(\theta = 0\)
- When \( x = 2 \): \(\sin^2 \theta = 1 \Rightarrow \theta = \pi/2\)

Compute the derivatives and transformed expressions:
- \( dx = 4 \sin \theta \cos \theta\, d\theta = 2 \sin 2\theta\, d\theta \)
- \( x^{1/2} = \sqrt{2} \sin \theta \)
- \( 2-x = 2(1 - \sin^2 \theta) = 2 \cos^2 \theta \Rightarrow (2-x)^{-1/2} = (2 \cos^2 \theta)^{-1/2} = \frac{1}{\sqrt{2} \cos \theta} \)
- \( \sqrt{x(2-x)} = \sqrt{2 \sin^2 \theta \cdot 2 \cos^2 \theta} = 2 \sin\theta \cos\theta = \sin 2\theta \)

Substitute all into the integral:
\[
I = \int_0^{\pi/2} 
\left[\sqrt{2} \sin\theta \cdot \frac{1}{\sqrt{2} \cos\theta}\right] \cos(\sin 2\theta) \cdot 2\sin 2\theta d\theta
\]

Now simplify:

- \( \sqrt{2} / \sqrt{2} = 1 \)
- \( \sin\theta / \cos\theta = \tan\theta \)
- \( 2\sin 2\theta = 4\sin\theta\cos\theta \)

But since \( dx = 4 \sin \theta \cos \theta d\theta \), we get:

\[
I = \int_0^{\pi/2} \frac{\sin \theta}{\cos \theta} \cos(\sin 2\theta) \cdot 4\sin\theta \cos\theta d\theta
\]
\[
= 4 \int_0^{\pi/2} \frac{\sin\theta}{\cos\theta} \sin\theta \cos\theta \cos(\sin 2\theta) d\theta
\]
\[
= 4 \int_0^{\pi/2} \sin^2\theta \cos(\sin 2\theta) d\theta
\]

Recall that \( \sin 2\theta = 2\sin\theta\cos\theta \), but it is more convenient to keep as is for now.

### Step 2: Reduce using double-angle identities

Use \( \sin^2 \theta = \frac{1 - \cos 2\theta}{2} \) to further simplify:

\[
I = 4 \int_0^{\pi/2} \frac{1 - \cos 2\theta}{2} \cos(\sin 2\theta) d\theta
= 2 \int_0^{\pi/2} [1 - \cos 2\theta] \cos(\sin 2\theta) d\theta
\]
\[
= 2 \int_0^{\pi/2} \cos(\sin 2\theta) d\theta - 2 \int_0^{\pi/2} \cos 2\theta\ \cos(\sin 2\theta) d\theta
\]

### Step 3: Express cos 2θ cos(sin 2θ) using product-to-sum

\[
\cos 2\theta\ \cos(\sin 2\theta)
= \frac{1}{2} \left[ \cos(2\theta + \sin 2\theta) + \cos(2\theta - \sin 2\theta) \right]
\]

Thus,

\[
I = 2 \int_0^{\pi/2} \cos(\sin 2\theta) d\theta
- \int_0^{\pi/2} \left[ \cos(2\theta + \sin 2\theta) + \cos(2\theta - \sin 2\theta) \right] d\theta
\]

\[
= 2 \int_0^{\pi/2} \cos(\sin 2\theta) d\theta
- \int_0^{\pi/2} \cos(2\theta + \sin 2\theta) d\theta
- \int_0^{\pi/2} \cos(2\theta - \sin 2\theta) d\theta
\]

### Step 4: Evaluation

These integrals do not have elementary closed forms directly, but we can relate them to Bessel functions.

Recall the integral representation of the Bessel function of the first kind:

\[
J_0(a) = \frac{1}{\pi} \int_0^\pi \cos(a \sin \phi) d\phi
\]

Now, in the first integral, we have \( \cos(\sin 2\theta) \), so \( a = 1 \) and the argument \( \sin 2\theta \).

Let us consider changing variable: \( \phi = 2\theta \), so as \( \theta \) goes from 0 to \( \pi/2 \), \( \phi \) goes from 0 to \( \pi \):
- \( d\theta = \frac{1}{2} d\phi \)

Thus:

\[
\int_0^{\pi/2} \cos(\sin 2\theta)\ d\theta = \frac{1}{2} \int_0^{\pi} \cos(\sin \phi)\ d\phi
\]
So:
\[
I = 2 \cdot \frac{1}{2} \int_0^{\pi} \cos(\sin \phi) d\phi - \int_0^{\pi/2} [\cos(2\theta + \sin 2\theta) + \cos(2\theta - \sin 2\theta)] d\theta
\]
\[
= \int_0^{\pi} \cos(\sin \phi) d\phi - \int_0^{\pi/2} [\cos(2\theta + \sin 2\theta) + \cos(2\theta - \sin 2\theta)] d\theta
\]

Now let's tackle the other two integrals.

Let’s focus on:

\[
\int_0^{\pi/2} \cos(2\theta \pm \sin 2\theta) d\theta
\]
Let’s use, for the minus sign, the change of variable \( \phi = 2\theta \):
- \( \theta = \frac{\phi}{2} \)
- \( d\theta = \frac{1}{2} d\phi \)
- as \( \theta \) varies from \( 0 \to \frac{\pi}{2} \), \( \phi \) varies from \( 0 \to \pi \)

So:

\[
\int_0^{\pi/2} \cos(2\theta \pm \sin 2\theta)\, d\theta = \frac{1}{2} \int_0^{\pi} \cos(\phi \pm \sin \phi)\, d\phi
\]

So:
\[
I = \int_0^\pi \cos(\sin \phi)\, d\phi
- \frac{1}{2}\int_0^{\pi} [\cos(\phi + \sin\phi) + \cos(\phi - \sin\phi)] d\phi
\]

Now, by the sum to product formula:

\[
\cos(A+B) + \cos(A-B) = 2 \cos A \cos B
\]

So,
\[
\cos(\phi + \sin\phi) + \cos(\phi - \sin\phi) = 2 \cos\phi\ \cos(\sin\phi)
\]

Therefore,

\[
I = \int_0^\pi \cos(\sin \phi)\, d\phi - \int_0^{\pi} \cos\phi \cos(\sin\phi) d\phi
\]

### Step 5: Express in terms of Bessel function

Now, let’s use the known properties of Bessel functions:

From a standard table:

\[
\int_0^\pi \cos(a \sin \theta)\ d\theta = \pi J_0(a)
\]

and

\[
\int_0^\pi \cos\theta \cos(a \sin \theta)\ d\theta = \pi J_1(a)
\]

Therefore,

\[
I = \pi J_0(1) - \pi J_1(1) = \pi[J_0(1) - J_1(1)]
\]

### Step 6: Numerical Approximation

The values:
- \( J_0(1) \approx 0.7651976866 \)
- \( J_1(1) \approx 0.4400505857 \)
- \( \pi \approx 3.1415926536 \)

Thus,
\[
J_0(1) - J_1(1) \approx 0.7651976866 - 0.4400505857 = 0.3251471009
\]
\[
I \approx 3.1415926536 \times 0.3251471009 = 1.0214966391
\]

Rounded to 10 decimal places: 1.0214966391

### Final Answers

- Exact answer: \( \pi[J_0(1) - J_1(1)] \)
- Numeric: 1.0214966391

```json
{"answer": "\\pi\\big[J_0(1)-J_1(1)\\big]", "numerical_answer": "1.0214966391"}
```