Let's solve the integral step by step:

\[
I = \int_0^{\frac{1}{2}} \left\lfloor \frac{1}{x} \right\rfloor \left\lceil \frac{1}{x} \right\rceil \ln\left(1 - \frac{1}{\left\lfloor \frac{1}{x} \right\rfloor^2}\right) dx
\]

### Step 1: Understanding the Integrand

For \(x \in (0, 1]\), \(\frac{1}{x}\) is greater than or equal to 1 and increases as \(x \to 0^{+}\).

- For \(x\) in the interval \(\left(\frac{1}{n+1}, \frac{1}{n}\right]\), \(\frac{1}{x}\) is in \([n, n+1)\), so:
  - \(\left\lfloor \frac{1}{x} \right\rfloor = n\)
  - \(\left\lceil \frac{1}{x} \right\rceil = n+1\)

For \(x = 1/n\), \(\frac{1}{x} = n\), so actually \(\lfloor 1/x \rfloor = \lceil 1/x \rceil = n\), but this is just a single point and does not affect the integral.

On \(x \in (0, 1/2]\), \(1/x\) ranges from 2 to \(\infty\).

So our sum is over \(n = 2, 3, 4, \ldots\).

### Step 2: Express as a Sum of Integrals over Each Interval

On each interval \(x \in \left(\frac{1}{n+1}, \frac{1}{n}\right]\):

- \(\left\lfloor \frac{1}{x} \right\rfloor = n\)
- \(\left\lceil \frac{1}{x} \right\rceil = n+1\)
- \(\ln\left( 1 - \frac{1}{\left\lfloor \frac{1}{x} \right\rfloor^2} \right) = \ln\left(1 - \frac{1}{n^2}\right)\)

Thus, the integral over this interval is:

\[
\int_{\frac{1}{n+1}}^{\frac{1}{n}} n(n+1) \ln\left(1-\frac{1}{n^2}\right) dx
\]

The total integral is:

\[
I = \sum_{n=2}^{\infty} n(n+1) \ln\left(1-\frac{1}{n^2}\right) \left( \frac{1}{n} - \frac{1}{n+1} \right)
\]

\[
= \sum_{n=2}^\infty n(n+1) \ln\left(1-\frac{1}{n^2}\right) \left( \frac{1}{n} - \frac{1}{n+1} \right)
\]

Now,

\[
\frac{1}{n} - \frac{1}{n+1} = \frac{1}{n(n+1)}
\]

So,

\[
I = \sum_{n=2}^{\infty} n(n+1) \ln\left(1-\frac{1}{n^2}\right) \cdot \frac{1}{n(n+1)}
= \sum_{n=2}^{\infty} \ln\left(1-\frac{1}{n^2}\right)
\]

### Step 3: Simplify the Logarithm

\[
\ln\left(1 - \frac{1}{n^2}\right) = \ln\left( \frac{n^2 - 1}{n^2}\right )
= \ln\left( \frac{n-1}{n} \cdot \frac{n+1}{n} \right )
= \ln\left( \frac{n-1}{n} \right ) + \ln\left( \frac{n+1}{n} \right )
\]

Thus,

\[
I = \sum_{n=2}^{\infty} \left[ \ln\left(\frac{n-1}{n}\right) + \ln\left(\frac{n+1}{n}\right) \right]
= \sum_{n=2}^\infty \ln\left( \frac{n-1}{n} \right ) + \sum_{n=2}^\infty \ln\left( \frac{n+1}{n} \right )
\]

\[
= \sum_{n=2}^\infty \ln\left( \frac{n-1}{n} \right ) + \sum_{n=2}^\infty \ln\left( \frac{n+1}{n} \right )
\]

\[
= \sum_{n=2}^\infty \ln\left( \frac{n-1}{n} \cdot \frac{n+1}{n} \right)
\]

But for clarity, we'll analyze the two sums separately:

#### First sum:

\[
S_1 = \sum_{n=2}^\infty \ln\left( \frac{n-1}{n} \right) = \sum_{n=2}^\infty [\ln(n-1) - \ln n] = \ln 1 - \ln 2 + \ln 2 - \ln 3 + \ln 3 - \ln 4 + \ldots
\]
So,

\[
S_1 = -\ln 2
\]
since all terms after the first cancel telescopically.

#### Second sum:

\[
S_2 = \sum_{n=2}^\infty \ln\left( \frac{n+1}{n} \right) = \sum_{n=2}^\infty [\ln(n+1) - \ln n] = \ln 3 - \ln 2 + \ln 4 - \ln 3 + \ln 5 - \ln 4 + \cdots
\]
So,

\[
S_2 = \lim_{N \to \infty} [\ln(N+1) - \ln 2] = \infty
\]

But let's combine the two:

\[
S = S_1 + S_2 = \sum_{n=2}^{\infty} \ln\left( \frac{n-1}{n} \right) + \sum_{n=2}^{\infty} \ln\left( \frac{n+1}{n} \right)
= \sum_{n=2}^\infty \ln\left( \frac{(n-1)(n+1)}{n^2} \right)
\]
\[
= \sum_{n=2}^{\infty} \ln\left( 1 - \frac{1}{n^2} \right)
\]

But as above, the sum diverges logarithmically, but in our definite integral, the sum of interest is:

\[
I = \sum_{n=2}^{\infty} \ln\left( 1 - \frac{1}{n^2} \right)
\]

But let's try a more subtle approach; perhaps, because the integral is over a finite domain, our sum converges as a value.

Let me be precise: for the upper limit \(x = \frac{1}{2}\), \( \frac{1}{x} = 2 \). Starting at \(n=2\), the interval stops at \(x = \frac{1}{2}\).

But for all \(n \ge 2\), the intervals \((\frac{1}{n+1}, \frac{1}{n}]\) are entirely inside \((0, \frac{1}{2}]\), since \(1/(n+1) < 1/2\) for all \(n \ge 2\).

Therefore, our sum is over \(n=2, 3, 4, ...\).

### Step 4: Explicit Summation

\[
I = \sum_{n=2}^{\infty} \ln\left( 1 - \frac{1}{n^2} \right)
= \sum_{n=2}^{\infty} \ln\left( \frac{n^2 - 1}{n^2} \right)
= \sum_{n=2}^{\infty} \ln \left( \frac{n-1}{n} \right ) + \ln \left( \frac{n+1}{n} \right )
\]
\[
= \sum_{n=2}^\infty \left [ \ln(n-1) - \ln n + \ln(n+1) - \ln n \right ]
= \sum_{n=2}^\infty ( \ln(n-1) + \ln(n+1) - 2 \ln n )
\]
\[
= \sum_{n=2}^\infty \ln(n-1) + \sum_{n=2}^\infty \ln(n+1) - 2 \sum_{n=2}^\infty \ln n
\]

Consider:

- \(\sum_{n=2}^\infty \ln(n-1) = \sum_{k=1}^\infty \ln k\)
- \(\sum_{n=2}^\infty \ln(n+1) = \sum_{k=3}^\infty \ln k\)
- \(\sum_{n=2}^\infty \ln n\) already as is.

So:

\[
I = \sum_{k=1}^\infty \ln k + \sum_{k=3}^\infty \ln k - 2 \sum_{n=2}^\infty \ln n
\]
\[
= \ln 1 + \ln 2 + \sum_{k=3}^\infty \ln k + \sum_{k=3}^\infty \ln k - 2 \left [ \ln 2 + \sum_{k=3}^{\infty} \ln k \right ]
\]
\[
= \ln 1 + \ln 2 + 2 \sum_{k=3}^\infty \ln k - 2 \ln 2 - 2 \sum_{k=3}^{\infty} \ln k
\]
\[
= \ln 1 + \ln 2 - 2 \ln 2
= -\ln 2
\]

Since \(\ln 1 = 0\), so:

\[
I = -\ln 2
\]

### Step 5: Numerical Value

\[
\boxed{
I = -\ln 2 \approx -0.6931471806
}
\]

(Rounded to 10 decimal places.)

---

### Final Answer

```json
{"answer": "-\\ln 2", "numerical_answer": "-0.6931471806"}
```