Let's compute the definite integral step by step:

\[
I = \int_{0}^{2} x^{-1/2} (2-x)^{-1/2} \left[1 - \frac{1}{2}x(2-x)\right] dx
\]

### Step 1: Simplify the integrand
First, observe that the integrand can be rewritten as:

\[
x^{-1/2} (2-x)^{-1/2} \left[1 - \frac{1}{2}x(2-x)\right] = \frac{1}{\sqrt{x(2-x)}} \left[1 - \frac{1}{2}x(2-x)\right]
\]

### Step 2: Substitute to simplify the integral
Let \( x = 2 \sin^2 \theta \), then \( dx = 4 \sin \theta \cos \theta d\theta \). The limits change as follows:
- When \( x = 0 \), \( \theta = 0 \).
- When \( x = 2 \), \( \theta = \pi/2 \).

Substitute \( x = 2 \sin^2 \theta \) into the integrand:

\[
\sqrt{x(2-x)} = \sqrt{2 \sin^2 \theta \cdot 2 \cos^2 \theta} = 2 \sin \theta \cos \theta
\]

\[
\frac{1}{\sqrt{x(2-x)}} = \frac{1}{2 \sin \theta \cos \theta}
\]

\[
\frac{1}{2}x(2-x) = \frac{1}{2} \cdot 2 \sin^2 \theta \cdot 2 \cos^2 \theta = 2 \sin^2 \theta \cos^2 \theta
\]

Thus, the integrand becomes:

\[
\frac{1}{2 \sin \theta \cos \theta} \left[1 - 2 \sin^2 \theta \cos^2 \theta\right] \cdot 4 \sin \theta \cos \theta d\theta
\]

Simplify:

\[
= 2 \left[1 - 2 \sin^2 \theta \cos^2 \theta\right] d\theta
\]

### Step 3: Compute the integral
Now, the integral becomes:

\[
I = 2 \int_{0}^{\pi/2} \left[1 - 2 \sin^2 \theta \cos^2 \theta\right] d\theta
\]

We can split this into two parts:

\[
I = 2 \left[ \int_{0}^{\pi/2} 1 \, d\theta - 2 \int_{0}^{\pi/2} \sin^2 \theta \cos^2 \theta \, d\theta \right]
\]

The first integral is straightforward:

\[
\int_{0}^{\pi/2} 1 \, d\theta = \frac{\pi}{2}
\]

For the second integral, use the identity \( \sin^2 \theta \cos^2 \theta = \frac{1}{4} \sin^2 2\theta \):

\[
\int_{0}^{\pi/2} \sin^2 \theta \cos^2 \theta \, d\theta = \frac{1}{4} \int_{0}^{\pi/2} \sin^2 2\theta \, d\theta
\]

Let \( \phi = 2\theta \), then \( d\theta = \frac{1}{2} d\phi \), and the limits become \( 0 \) to \( \pi \):

\[
\frac{1}{4} \int_{0}^{\pi} \sin^2 \phi \cdot \frac{1}{2} d\phi = \frac{1}{8} \int_{0}^{\pi} \sin^2 \phi \, d\phi
\]

Using the identity \( \sin^2 \phi = \frac{1 - \cos 2\phi}{2} \):

\[
\frac{1}{8} \int_{0}^{\pi} \frac{1 - \cos 2\phi}{2} d\phi = \frac{1}{16} \left[ \int_{0}^{\pi} 1 \, d\phi - \int_{0}^{\pi} \cos 2\phi \, d\phi \right]
\]

\[
= \frac{1}{16} \left[ \pi - 0 \right] = \frac{\pi}{16}
\]

Thus, the second part of \( I \) is:

\[
2 \cdot 2 \cdot \frac{\pi}{16} = \frac{\pi}{4}
\]

Putting it all together:

\[
I = 2 \left[ \frac{\pi}{2} - \frac{\pi}{4} \right] = 2 \cdot \frac{\pi}{4} = \frac{\pi}{2}
\]

### Step 4: Numerical approximation
The exact answer is \( \frac{\pi}{2} \), and its numerical approximation is:

\[
\frac{\pi}{2} \approx 1.5707963268
\]

### Final Answer
```json
{"answer": "\\frac{\\pi}{2}", "numerical_answer": "1.5707963268"}
```