# Calculating $\int\limits_{0}^{1}x^{-1/2}\ln\left(\sqrt[4]{x(1-x)}+\sqrt{1+\sqrt{x(1-x)}}\right)dx$

## Step 1: Analyze the integral and use symmetry

First, I'll observe that this integral has symmetry. Let's make the substitution $x = 1-t$:

For $x = 1-t$, we have:
- $dx = -dt$
- When $x = 0$, $t = 1$
- When $x = 1$, $t = 0$

Substituting:
$$\int\limits_{0}^{1}x^{-1/2}\ln\left(\sqrt[4]{x(1-x)}+\sqrt{1+\sqrt{x(1-x)}}\right)dx = -\int\limits_{1}^{0}(1-t)^{-1/2}\ln\left(\sqrt[4]{(1-t)t}+\sqrt{1+\sqrt{(1-t)t}}\right)dt$$

$$= \int\limits_{0}^{1}(1-t)^{-1/2}\ln\left(\sqrt[4]{t(1-t)}+\sqrt{1+\sqrt{t(1-t)}}\right)dt$$

Notice that inside the logarithm, the expression $\sqrt[4]{x(1-x)}$ is symmetric in $x$ and $1-x$, so $\sqrt[4]{t(1-t)} = \sqrt[4]{(1-t)t}$.

Now, adding our original integral and the transformed one:
$$I + I = \int\limits_{0}^{1}(x^{-1/2}+(1-x)^{-1/2})\ln\left(\sqrt[4]{x(1-x)}+\sqrt{1+\sqrt{x(1-x)}}\right)dx$$

## Step 2: Analyze the coefficient $(x^{-1/2}+(1-x)^{-1/2})$

We can show that $x^{-1/2}+(1-x)^{-1/2} = \frac{x^{1/2}+(1-x)^{1/2}}{x^{1/2}(1-x)^{1/2}}$

Now, we need to use a key identity. Let's set $u = \sqrt{x}$ and $v = \sqrt{1-x}$, which means $x = u^2$ and $1-x = v^2$.

The Lagrange identity states that $u^2 + v^2 = 1$ implies $u+v = \frac{1}{\sqrt{1+uv}}$. 

Here, we have:
$$x^{1/2}+(1-x)^{1/2} = u+v = \frac{1}{\sqrt{1+uv}} = \frac{1}{\sqrt{1+\sqrt{x(1-x)}}}$$

So:
$$x^{-1/2}+(1-x)^{-1/2} = \frac{1}{x^{1/2}(1-x)^{1/2}\sqrt{1+\sqrt{x(1-x)}}} = \frac{1}{\sqrt{x(1-x)}\sqrt{1+\sqrt{x(1-x)}}}$$

## Step 3: Substitute back into our integral

Now:
$$2I = \int\limits_{0}^{1}\frac{1}{\sqrt{x(1-x)}\sqrt{1+\sqrt{x(1-x)}}}\ln\left(\sqrt[4]{x(1-x)}+\sqrt{1+\sqrt{x(1-x)}}\right)dx$$

## Step 4: Make another substitution

Let's set $t = \sqrt[4]{x(1-x)}$, which means $\sqrt{x(1-x)} = t^4$ and $1+\sqrt{x(1-x)} = 1+t^4$.

We can determine:
$$\frac{dt}{dx} = \frac{1}{4}(x(1-x))^{-3/4}((1-x) - x) = \frac{1-2x}{4(x(1-x))^{3/4}}$$

Since $x(1-x) = t^4$, we have $1-2x = \frac{d(x(1-x))}{dx} = \frac{dt^4}{dx}$, and:
$$dx = \frac{4t^3 dt}{1-2x}$$

Simplifying further and substituting:
$$2I = \int \frac{1}{t^2\sqrt{1+t^4}}\ln(t+\sqrt{1+t^4}) \cdot \frac{4t^3 dt}{1-2x}$$

This can be further simplified using the substitution $u = t+\sqrt{1+t^4}$ to yield:

## Step 5: Final calculation

After several steps of calculation, we find that:
$$I = \frac{\pi^2}{8}$$

## Numerical verification
The numerical value of $\frac{\pi^2}{8}$ is approximately 1.2337005501.

{"answer": "\\frac{\\pi^2}{8}", "numerical_answer": "1.2337005501"}