# Evaluating $\large\int_0^\infty\frac{\tanh(x)}{\exp(x)}dx$

## Step 1: Rewrite the integrand

Recall that $\tanh(x) = \frac{e^x - e^{-x}}{e^x + e^{-x}}$

So we have:
$$\int_0^\infty\frac{\tanh(x)}{\exp(x)}dx = \int_0^\infty\frac{1}{e^x}\cdot\frac{e^x - e^{-x}}{e^x + e^{-x}}dx = \int_0^\infty\frac{e^x - e^{-x}}{e^{2x} + 1}dx$$

## Step 2: Substitute $u = e^x$

Let $u = e^x$, then $dx = \frac{du}{u}$, and when $x = 0$, $u = 1$; when $x \to \infty$, $u \to \infty$.

The integral becomes:
$$\int_1^\infty\frac{u - \frac{1}{u}}{u^2 + 1}\cdot\frac{du}{u} = \int_1^\infty\frac{u^2 - 1}{u(u^2 + 1)}du$$

## Step 3: Partial fraction decomposition

Let's decompose $\frac{u^2 - 1}{u(u^2 + 1)}$:

$$\frac{u^2 - 1}{u(u^2 + 1)} = \frac{A}{u} + \frac{Bu + C}{u^2 + 1}$$

Multiplying both sides by $u(u^2 + 1)$:
$$u^2 - 1 = A(u^2 + 1) + (Bu + C)u$$

Expanding:
$$u^2 - 1 = Au^2 + A + Bu^2 + Cu$$

Comparing coefficients:
- $u^2$: $1 = A + B$
- $u^1$: $0 = C$
- $u^0$: $-1 = A$

From this we get $A = -1$, $C = 0$, and $B = 2$.

So:
$$\frac{u^2 - 1}{u(u^2 + 1)} = -\frac{1}{u} + \frac{2u}{u^2 + 1}$$

## Step 4: Integrate each term

Our integral becomes:
$$\int_1^\infty\left(-\frac{1}{u} + \frac{2u}{u^2 + 1}\right)du = -\int_1^\infty\frac{1}{u}du + 2\int_1^\infty\frac{u}{u^2 + 1}du$$

For the first term:
$$-\int_1^\infty\frac{1}{u}du = -[\ln|u|]_1^\infty = -(\ln(\infty) - \ln(1)) = -\infty$$

However, this suggests there's an issue with our decomposition. Let's double-check.

Actually, we can verify that:
$$\frac{u^2 - 1}{u(u^2 + 1)} = \frac{u^2 + 1 - 2}{u(u^2 + 1)} = \frac{1}{u} - \frac{2}{u(u^2 + 1)}$$

Now, let's further decompose $\frac{2}{u(u^2 + 1)}$:
$$\frac{2}{u(u^2 + 1)} = \frac{A}{u} + \frac{Bu + C}{u^2 + 1}$$

Multiplying both sides by $u(u^2 + 1)$:
$$2 = A(u^2 + 1) + (Bu + C)u$$

Comparing coefficients:
- $u^2$: $0 = A + B$
- $u^1$: $0 = C$
- $u^0$: $2 = A$

So $A = 2$, $C = 0$, and $B = -2$.

This gives us:
$$\frac{2}{u(u^2 + 1)} = \frac{2}{u} - \frac{2u}{u^2 + 1}$$

Correcting our original decomposition:
$$\frac{u^2 - 1}{u(u^2 + 1)} = \frac{1}{u} - \frac{2}{u} + \frac{2u}{u^2 + 1} = -\frac{1}{u} + \frac{2u}{u^2 + 1}$$

This matches our earlier result, so our decomposition was correct.

## Step 5: Re-examine the integral

Let's reconsider the integral directly:

$$\int_0^\infty\frac{\tanh(x)}{e^x}dx = \int_0^\infty\frac{1 - e^{-2x}}{1 + e^{-2x}}e^{-x}dx$$

Let $u = e^{-2x}$, then $dx = -\frac{du}{2u}$, and when $x = 0$, $u = 1$; when $x \to \infty$, $u \to 0$.

The integral becomes:
$$\int_1^0\frac{1 - u}{1 + u}e^{-x}\left(-\frac{du}{2u}\right) = \frac{1}{2}\int_0^1\frac{1 - u}{1 + u}e^{-x}\frac{du}{u}$$

Now we need to express $e^{-x}$ in terms of $u$:
$e^{-x} = e^{-x} = (e^{-2x})^{1/2} = u^{1/2}$

So our integral is:
$$\frac{1}{2}\int_0^1\frac{1 - u}{1 + u}u^{1/2}\frac{du}{u} = \frac{1}{2}\int_0^1\frac{1 - u}{1 + u}u^{-1/2}du$$

## Step 6: Another approach using substitution

Let's restart with a simpler approach.

We have $\tanh(x) = \frac{e^x - e^{-x}}{e^x + e^{-x}}$, so:

$$\int_0^\infty\frac{\tanh(x)}{e^x}dx = \int_0^\infty\frac{e^x - e^{-x}}{e^x + e^{-x}} \cdot e^{-x}dx = \int_0^\infty\frac{1 - e^{-2x}}{1 + e^{-2x}}e^{-x}dx$$

Let $t = e^{-x}$, then $dx = -\frac{dt}{t}$, and when $x = 0$, $t = 1$; when $x \to \infty$, $t \to 0$.

The integral becomes:
$$\int_1^0\frac{1 - t^2}{1 + t^2}t\left(-\frac{dt}{t}\right) = \int_0^1\frac{1 - t^2}{1 + t^2}dt$$

Now, we can split this:
$$\int_0^1\frac{1 - t^2}{1 + t^2}dt = \int_0^1\frac{dt}{1 + t^2} - \int_0^1\frac{t^2}{1 + t^2}dt$$

The first integral is $\arctan(t)$ evaluated from 0 to 1:
$$\int_0^1\frac{dt}{1 + t^2} = [\arctan(t)]_0^1 = \arctan(1) - \arctan(0) = \frac{\pi}{4} - 0 = \frac{\pi}{4}$$

For the second integral, we can rewrite it:
$$\int_0^1\frac{t^2}{1 + t^2}dt = \int_0^1\left(1 - \frac{1}{1 + t^2}\right)dt = \int_0^1 dt - \int_0^1\frac{dt}{1 + t^2}$$

The integral $\int_0^1 dt = 1$ and $\int_0^1\frac{dt}{1 + t^2} = \frac{\pi}{4}$ as we calculated above.

So:
$$\int_0^1\frac{t^2}{1 + t^2}dt = 1 - \frac{\pi}{4}$$

Going back to our original split:
$$\int_0^1\frac{1 - t^2}{1 + t^2}dt = \frac{\pi}{4} - (1 - \frac{\pi}{4}) = \frac{\pi}{4} - 1 + \frac{\pi}{4} = \frac{\pi}{2} - 1$$

## Final Answer

The definite integral $\int_0^\infty\frac{\tanh(x)}{\exp(x)}dx = \frac{\pi}{2} - 1$

Numerical approximation: $\frac{\pi}{2} - 1 \approx 0.5707963268$

{"answer": "\\frac{\\pi}{2} - 1", "numerical_answer": "0.5707963268"}