We wish to evaluate

  I = ∫₀¹ (e^(eˣ) − e^(eˣ − x)) dx.

Step 1. Split the integral:
  I = ∫₀¹ e^(eˣ) dx − ∫₀¹ e^(eˣ − x) dx.

Step 2. Write the second term in an equivalent form:
  e^(eˣ − x) = e^(eˣ) · e^(−x).
Thus,
  I = ∫₀¹ e^(eˣ) dx − ∫₀¹ e^(eˣ) e^(−x) dx.

Step 3. Substitute u = eˣ. Then du = eˣ dx, so that dx = du/u. When x = 0, u = 1 and when x = 1, u = e.
- For the first integral:
  ∫₀¹ e^(eˣ) dx = ∫₁ᵉ e^(u) (du/u) = ∫₁ᵉ (e^(u)/u) du.
- For the second integral note that e^(−x) = 1/eˣ = 1/u, so:
  ∫₀¹ e^(eˣ) e^(−x) dx = ∫₁ᵉ e^(u) (1/u) (du/u) = ∫₁ᵉ (e^(u)/u²) du.

Thus the integral becomes:
  I = ∫₁ᵉ (e^(u)/u) du − ∫₁ᵉ (e^(u)/u²) du = ∫₁ᵉ e^(u) (1/u − 1/u²) du.
We can combine the terms in the integrand:
  1/u − 1/u² = (u − 1)/u²,
so
  I = ∫₁ᵉ e^(u) (u − 1)/u² du.

Step 4. Notice that the derivative of (e^(u)/u) is computed by the quotient rule:
  d/du (e^(u)/u) = (e^(u)·u − e^(u))/(u²) = e^(u) (u − 1)/u².
Thus, the integrand is exactly the derivative of (e^(u)/u). Therefore,
  I = [e^(u)/u] evaluated from u = 1 to u = e.

Step 5. Evaluate the antiderivative at the bounds:
  At u = e: e^(e)/e = e^(e − 1).
  At u = 1: e^(1)/1 = e.
So,
  I = e^(e − 1) − e.

Step 6. Numerical approximation:
Using e ≈ 2.7182818285,
  e − 1 ≈ 1.7182818285,
and then e^(e − 1) = e^(1.7182818285) ≈ 5.5749415160.
Thus,
  I ≈ 5.5749415160 − 2.7182818285 ≈ 2.8566596875.

The final answer is provided below in the requested JSON format.

{"answer": "$e^{e-1} - e$", "numerical_answer": "2.8566596875"}