Let's proceed step by step:

**1. Compute the integral analytically.**

Let
\[
I = \int_{-1}^0 5(x^6 + x)^4 \, dx
\]

Let’s make the substitution:
Let \( u = x^6 + x \). Then
\[
\frac{du}{dx} = 6x^5 + 1
\]
But this is more complicated than the integrand, so instead let's expand \((x^6 + x)^4\) using the binomial theorem.

\((x^6 + x)^4 = \sum_{k=0}^{4} \binom{4}{k} (x^6)^{4-k} (x)^k = \sum_{k=0}^4 \binom{4}{k} x^{6(4-k)} x^{k}\)

But that's not quite correct; the exponents on \(x\) should be \(6(4-k)+k = 24-5k\):

\begin{align*}
(x^6 + x)^4 &= \sum_{k=0}^4 \binom{4}{k} (x^6)^{4-k} (x)^{k} \\
&= \sum_{k=0}^4 \binom{4}{k} x^{6(4-k) + k} \\
&= \sum_{k=0}^4 \binom{4}{k} x^{24-6k + k} \\
&= \sum_{k=0}^4 \binom{4}{k} x^{24 - 5k} \\
\end{align*}

Therefore,
\[
I = 5 \int_{-1}^{0} (x^6 + x)^4 dx = 5 \int_{-1}^0 \left[ \sum_{k=0}^4 \binom{4}{k} x^{24-5k} \right] dx
= 5 \sum_{k=0}^4 \binom{4}{k} \int_{-1}^0 x^{24 - 5k} dx
\]

Each term is a simple power:
\[
\int_{-1}^0 x^n dx = \frac{1}{n+1} \left[ x^{n+1} \right]_{-1}^0 = \frac{0^{n+1} - (-1)^{n+1}}{n+1} = \frac{-(-1)^{n+1}}{n+1} = \frac{(-1)^n}{n+1}
\]
because \( -(-1)^{n+1} = (-1)^n \).

Now let's compute each term for \(k = 0, 1, 2, 3, 4\):

- For \(k = 0\): \(\binom{4}{0} = 1\), exponent is \(24\).
- For \(k = 1\): \(\binom{4}{1} = 4\), exponent is \(19\).
- For \(k = 2\): \(\binom{4}{2} = 6\), exponent is \(14\).
- For \(k = 3\): \(\binom{4}{3} = 4\), exponent is \(9\).
- For \(k = 4\): \(\binom{4}{4} = 1\), exponent is \(4\).

So:

\[
I = 5 \left[
1 \cdot \frac{(-1)^{24}}{25} +
4 \cdot \frac{(-1)^{19}}{20} +
6 \cdot \frac{(-1)^{14}}{15} +
4 \cdot \frac{(-1)^9}{10} +
1 \cdot \frac{(-1)^4}{5}
\right]
\]

Now compute the signs:
- \((-1)^{24} = 1\)
- \((-1)^{19} = -1\)
- \((-1)^{14} = 1\)
- \((-1)^9 = -1\)
- \((-1)^4 = 1\)

So:

\[
I = 5 \left[
\frac{1}{25}
-4 \cdot \frac{1}{20}
+6 \cdot \frac{1}{15}
-4 \cdot \frac{1}{10}
+\frac{1}{5}
\right]
\]

Let’s write all with a common denominator. The denominators are: 25, 20, 15, 10, and 5.

The least common multiple is 300.

Express each fraction over 300:

- \(\frac{1}{25} = \frac{12}{300}\)
- \(\frac{4}{20} = \frac{4}{20} = \frac{60}{300}\)
- \(\frac{6}{15} = \frac{2}{5} = \frac{120}{300}\)
- \(\frac{4}{10} = \frac{2}{5} = \frac{120}{300}\)
- \(\frac{1}{5} = \frac{60}{300}\)

Combining with signs:

\[
I = 5 \left[
\frac{12}{300}
- \frac{60}{300}
+ \frac{120}{300}
- \frac{120}{300}
+ \frac{60}{300}
\right]
= 5 \left[
\frac{12 - 60 + 120 - 120 + 60}{300}
\right]
= 5 \left[
\frac{12 - 60 + 60}{300}
\right]
= 5 \left[
\frac{12}{300}
\right]
= 5 \cdot \frac{1}{25}
= \frac{1}{5}
\]

**2. Final answer (analytical):**
\[
I = \frac{1}{5}
\]

**3. Numerical approximation:**
\[
\frac{1}{5} = 0.2
\]

Rounded to 10 decimal places: \(0.2000000000\)

**4. JSON output:**
```json
{"answer": "\\frac{1}{5}", "numerical_answer": "0.2000000000"}
```