We wish to evaluate

  I = ∫₀¹ [e^(eˣ) – e^(eˣ – x)] dx.

Step 1. Rewrite the integrand

Notice that
  e^(eˣ – x) = e^(eˣ) · e^(–x).
So the integrand can be written as
  e^(eˣ) – e^(eˣ – x) = e^(eˣ)[1 – e^(–x)].

That is,
  I = ∫₀¹ e^(eˣ)[1 – e^(–x)] dx.

Step 2. Apply the substitution u = eˣ

Let
  u = eˣ  ⇒  du/dx = eˣ  ⇒  dx = du/u.
When x = 0, u = e⁰ = 1.
When x = 1, u = e¹ = e.
Also, note that e^(eˣ) = eᵘ and e^(–x) = 1/eˣ = 1/u.

Thus the integral becomes
  I = ∫ᵤ₌₁ᵉ eᵘ [1 – 1/u] · (du/u)
    = ∫₁ᵉ [eᵘ/u]·[1 – 1/u] du
    = ∫₁ᵉ [eᵘ/u – eᵘ/u²] du.

Step 3. Recognize an exact derivative

Let’s consider the derivative of the function F(u) = eᵘ/u. Differentiate using the quotient rule:
  F′(u) = (eᵘ·u – eᵘ)/(u²) = eᵘ (u – 1)/u².
But note that
  eᵘ (u – 1)/u² = eᵘ/u – eᵘ/u²,
which exactly matches the integrand.

Thus,
  d/du (eᵘ/u) = eᵘ/u – eᵘ/u².

Step 4. Evaluate the integral

Since the integrand is the derivative of eᵘ/u, we have
  I = [eᵘ/u] evaluated from u = 1 to u = e.
That is,
  I = (e^(e)/e) – (e¹/1) = e^(e–1) – e.

Step 5. Obtain a numerical approximation

We now approximate I = e^(e–1) – e. Using
  e = 2.718281828459045…,
we compute the exponent:
  e – 1 = 1.718281828459045…
Then,
  e^(e–1) = exp(1.718281828459045) ≈ 5.5755518 (approx).
Thus,
  I ≈ 5.5755518 – 2.718281828459045 ≈ 2.857269972.

Rounded to 10 decimal places, the numerical result is 2.8572699720.

Final Answer in JSON format:
{"answer": "e^{e-1} - e", "numerical_answer": "2.8572699720"}