

To solve the definite integral \(\int_{0}^{2} x^{-1/2}(2-x)^{-1/2} \cosh\left(\sqrt{x(2-x)}\right) \, dx\), we proceed as follows:

### Step 1: Simplify the Integrand via Substitution
First, rewrite the integrand using \(x(2-x) = 2x - x^2\). Completing the square, we have \(2x - x^2 = 1 - (x-1)^2\). Let \(x = 1 + \sin\theta\), so \(dx = \cos\theta \, d\theta\). When \(x=0\), \(\theta = -\pi/2\); when \(x=2\), \(\theta = \pi/2\). Substituting:
- \(x(2-x) = 1 - \sin^2\theta = \cos^2\theta\), so \(\sqrt{x(2-x)} = \cos\theta\).
- \(x^{-1/2}(2-x)^{-1/2} = (\cos^2\theta)^{-1/2} = 1/\cos\theta\).

The integral becomes:
\[
\int_{-\pi/2}^{\pi/2} \frac{1}{\cos\theta} \cosh(\cos\theta) \cdot \cos\theta \, d\theta = \int_{-\pi/2}^{\pi/2} \cosh(\cos\theta) \, d\theta.
\]

### Step 2: Use Symmetry and Bessel Function Identity
The integrand \(\cosh(\cos\theta)\) is even, so the integral over \([-π/2, π/2]\) equals \(2 \int_{0}^{\pi/2} \cosh(\cos\theta) \, d\theta\). 

Recall the integral representation of the modified Bessel function of the first kind, \(I_0(z)\):
\[
I_0(z) = \frac{1}{\pi} \int_{0}^{\pi} \cosh(z \cos\theta) \, d\theta.
\]
Splitting the integral over \([0, π]\) into \([0, π/2]\) and \([π/2, π]\) (using symmetry), we find:
\[
\int_{0}^{\pi/2} \cosh(z \cos\theta) \, d\theta = \frac{\pi}{2} I_0(z).
\]
Setting \(z=1\), we get:
\[
\int_{0}^{\pi/2} \cosh(\cos\theta) \, d\theta = \frac{\pi}{2} I_0(1).
\]

### Step 3: Combine Results
The original integral simplifies to:
\[
2 \cdot \frac{\pi}{2} I_0(1) = \pi I_0(1).
\]

### Step 4: Numerical Approximation
The modified Bessel function \(I_0(1) \approx 1.2660658777520088\). Thus:
\[
\pi I_0(1) \approx 3.141592653589793 \times 1.2660658777520088 \approx 3.9774628561.
\]

{"answer": "\(\pi I_0(1)\)", "numerical_answer": "3.9774628561"}