We wish to evaluate

  I = ∫₀¹ arctan(√(x(1 – x))) dx.

A good strategy is to use the substitution

  x = sin²θ,  0 ≤ θ ≤ π/2.

Then

  dx = 2 sinθ cosθ dθ  and  √(x(1 – x)) = √(sin²θ cos²θ) = sinθ cosθ.

Thus the integral becomes

  I = ∫₀^(π/2) arctan(sinθ cosθ) · 2 sinθ cosθ dθ.

Since sinθ cosθ = (1/2) sin2θ, we write

  I = 2 ∫₀^(π/2) arctan((1/2) sin2θ) sinθ cosθ dθ
    = 2 ∫₀^(π/2) arctan((1/2) sin2θ) · (1/2) sin2θ dθ
    = ∫₀^(π/2) arctan((1/2) sin2θ) sin2θ dθ.

Now make the substitution

  u = 2θ,  so that dθ = du/2,
  u: 0 → π.

Then

  I = ∫₀^π arctan((1/2) sin u) sin u (du/2)
    = ½ ∫₀^π arctan((1/2) sin u) sin u du.

Thus, if we set

  J = ∫₀^π arctan((1/2) sin u) sin u du,
then
  I = J/2.

To compute J we introduce a parameter. More generally, define

  I(α) = ∫₀^π arctan(α sin u) sin u du.
Then our desired J is I(1/2).

Step 1. Differentiate I(α) with respect to α:
  d/dα [arctan(α sin u)] = sin u/(1 + α² sin²u).
Thus,
  I′(α) = ∫₀^π [sin u/(1 + α² sin²u)] sin u du = ∫₀^π sin²u/(1 + α² sin²u) du.

Step 2. Rewrite the integrand by noticing that
  sin²u/(1 + α² sin²u) = 1/α² [ (1 + α² sin²u – 1)/(1 + α² sin²u) ]
             = 1/α² [1 – 1/(1 + α² sin²u)].
Thus,
  I′(α) = 1/α² [ ∫₀^π 1 du – ∫₀^π 1/(1 + α² sin²u) du ].

A standard result is
  ∫₀^π du/(1 + α² sin²u) = π/√(1 + α²).

So we have
  I′(α) = [π/α²] [1 – 1/√(1 + α²)].

Step 3. Integrate with respect to α from 0 to 1/2. Since I(0) = 0 we get
  I(1/2) = ∫₀^(1/2) I′(α) dα = π ∫₀^(1/2) [1 – 1/√(1 + α²)]/α² dα.

This integral appears to be singular at α = 0, but a closer look shows that the singular parts cancel. To evaluate it we write the integrals separately:
  ∫ (1/α²) dα = –1/α  and
  ∫ 1/(α²√{1 + α²}) dα.
A substitution shows that
  ∫ dα/(α²√{1 + α²}) = –√(1 + α²)/α + C.
Thus,
  ∫₀^(1/2) [1 – 1/√(1 + α²)]/α² dα
    = [ –1/α + √(1 + α²)/α ] evaluated from 0 to 1/2
    = ( √(1 + (1/2)²) – 1 )/(1/2)       (the limits at 0 cancel).
Since (1/2)² = 1/4, we have √(1 + 1/4) = √(5/4) = (√5)/2. Therefore,
  I(1/2) = π · ( ( (√5)/2 – 1 )/(1/2) ) = π · 2 ( (√5)/2 – 1 )
       = π (√5 – 2).

Recall that J = I(1/2) and our desired integral was I = J/2. Hence,
  I = π (√5 – 2)/2.

Thus the exact answer is
  (π/2)(√5 – 2).

Step 4. Now we compute a numerical approximation. We have:
  √5 ≈ 2.2360679775  so  √5 – 2 ≈ 0.2360679775.
Multiplying by π and dividing by 2 gives:
  I ≈ (3.1415926536 × 0.2360679775)/2 ≈ 0.7415311856/2 ≈ 0.3707655928.

Finally, we output the result in the required JSON format.

{"answer": "\\frac{\\pi}{2}(\\sqrt{5}-2)", "numerical_answer": "0.3707655928"}