To solve the definite integral \(\int_0^6 \left( x + (x-3)^7 + \sin(x-3) \right) \, dx\), we will break it down into three separate integrals and solve each one individually.

### Step 1: Compute the integral analytically

First, we split the integral into three parts:
\[
\int_0^6 \left( x + (x-3)^7 + \sin(x-3) \right) \, dx = \int_0^6 x \, dx + \int_0^6 (x-3)^7 \, dx + \int_0^6 \sin(x-3) \, dx
\]

#### Integral 1: \(\int_0^6 x \, dx\)

This is a straightforward integral:
\[
\int_0^6 x \, dx = \left[ \frac{x^2}{2} \right]_0^6 = \frac{6^2}{2} - \frac{0^2}{2} = \frac{36}{2} = 18
\]

#### Integral 2: \(\int_0^6 (x-3)^7 \, dx\)

We use the substitution \(u = x - 3\), hence \(du = dx\). When \(x = 0\), \(u = -3\), and when \(x = 6\), \(u = 3\). The integral becomes:
\[
\int_{-3}^3 u^7 \, du
\]
Since \(u^7\) is an odd function, the integral of an odd function over a symmetric interval around zero is zero:
\[
\int_{-3}^3 u^7 \, du = 0
\]

#### Integral 3: \(\int_0^6 \sin(x-3) \, dx\)

Again, we use the substitution \(u = x - 3\), hence \(du = dx\). When \(x = 0\), \(u = -3\), and when \(x = 6\), \(u = 3\). The integral becomes:
\[
\int_{-3}^3 \sin(u) \, du
\]
Since \(\sin(u)\) is an odd function, the integral of an odd function over a symmetric interval around zero is zero:
\[
\int_{-3}^3 \sin(u) \, du = 0
\]

### Step 2: Combine the results

Combining the results of the three integrals, we get:
\[
\int_0^6 \left( x + (x-3)^7 + \sin(x-3) \right) \, dx = 18 + 0 + 0 = 18
\]

### Step 3: Numerical approximation

The exact answer is already a simple number, so the numerical approximation is the same:
\[
18.0000000000
\]

### Step 4: Output the final answer in JSON format

\[
\boxed{
\begin{aligned}
&\text{"answer": "18",} \\
&\text{"numerical_answer": "18.0000000000"}
\end{aligned}
}
\]