To solve the definite integral \(\int\limits_{0}^{\infty}\frac{x^{2}}{e^x-1}\left[2^{3}\sinh\left(0.5x\right)-\sinh\left(0.25x\right)\right]dx\), we will follow the steps outlined.

### Step 1: Simplify the integrand

First, let's simplify the expression inside the integral:
\[ 2^3 \sinh(0.5x) - \sinh(0.25x) = 8 \sinh(0.5x) - \sinh(0.25x). \]

Recall the definition of the hyperbolic sine function:
\[ \sinh(y) = \frac{e^y - e^{-y}}{2}. \]

Thus,
\[ \sinh(0.5x) = \frac{e^{0.5x} - e^{-0.5x}}{2}, \]
\[ \sinh(0.25x) = \frac{e^{0.25x} - e^{-0.25x}}{2}. \]

Substituting these into the integrand, we get:
\[ 8 \sinh(0.5x) - \sinh(0.25x) = 8 \cdot \frac{e^{0.5x} - e^{-0.5x}}{2} - \frac{e^{0.25x} - e^{-0.25x}}{2} \]
\[ = 4(e^{0.5x} - e^{-0.5x}) - \frac{e^{0.25x} - e^{-0.25x}}{2}. \]

### Step 2: Split the integral

Now, we split the integral into two parts:
\[ \int\limits_{0}^{\infty} \frac{x^2}{e^x - 1} \left[ 4(e^{0.5x} - e^{-0.5x}) - \frac{e^{0.25x} - e^{-0.25x}}{2} \right] dx. \]

This can be written as:
\[ 4 \int\limits_{0}^{\infty} \frac{x^2 (e^{0.5x} - e^{-0.5x})}{e^x - 1} dx - \frac{1}{2} \int\limits_{0}^{\infty} \frac{x^2 (e^{0.25x} - e^{-0.25x})}{e^x - 1} dx. \]

### Step 3: Use known integral results

We use the known result for integrals of the form:
\[ \int\limits_{0}^{\infty} \frac{x^2 e^{-ax}}{e^x - 1} dx = 2 \zeta(3) - 2a^2 \zeta(2) + 2a^3 \ln(2), \]
where \(\zeta(s)\) is the Riemann zeta function.

For \(a = 0.5\):
\[ \int\limits_{0}^{\infty} \frac{x^2 e^{-0.5x}}{e^x - 1} dx = 2 \zeta(3) - 2(0.5)^2 \zeta(2) + 2(0.5)^3 \ln(2). \]

For \(a = -0.5\):
\[ \int\limits_{0}^{\infty} \frac{x^2 e^{0.5x}}{e^x - 1} dx = 2 \zeta(3) - 2(-0.5)^2 \zeta(2) + 2(-0.5)^3 \ln(2). \]

Combining these:
\[ \int\limits_{0}^{\infty} \frac{x^2 (e^{0.5x} - e^{-0.5x})}{e^x - 1} dx = 2 \zeta(3) - 2(0.5)^2 \zeta(2) + 2(0.5)^3 \ln(2) - (2 \zeta(3) - 2(0.5)^2 \zeta(2) - 2(0.5)^3 \ln(2)) \]
\[ = 4(0.5)^3 \ln(2) = 4 \cdot 0.125 \ln(2) = 0.5 \ln(2). \]

Similarly, for \(a = 0.25\):
\[ \int\limits_{0}^{\infty} \frac{x^2 e^{-0.25x}}{e^x - 1} dx = 2 \zeta(3) - 2(0.25)^2 \zeta(2) + 2(0.25)^3 \ln(2). \]

For \(a = -0.25\):
\[ \int\limits_{0}^{\infty} \frac{x^2 e^{0.25x}}{e^x - 1} dx = 2 \zeta(3) - 2(-0.25)^2 \zeta(2) + 2(-0.25)^3 \ln(2). \]

Combining these:
\[ \int\limits_{0}^{\infty} \frac{x^2 (e^{0.25x} - e^{-0.25x})}{e^x - 1} dx = 2 \zeta(3) - 2(0.25)^2 \zeta(2) + 2(0.25)^3 \ln(2) - (2 \zeta(3) - 2(0.25)^2 \zeta(2) - 2(0.25)^3 \ln(2)) \]
\[ = 4(0.25)^3 \ln(2) = 4 \cdot 0.015625 \ln(2) = 0.0625 \ln(2). \]

### Step 4: Combine the results

Combining the results from the integrals:
\[ 4 \cdot 0.5 \ln(2) - \frac{1}{2} \cdot 0.0625 \ln(2) = 2 \ln(2) - 0.03125 \ln(2) = 1.96875 \ln(2). \]

### Step 5: Numerical approximation

Using the approximation \(\ln(2) \approx 0.69314718056\):
\[ 1.96875 \ln(2) \approx 1.96875 \times 0.69314718056 \approx 1.365044921875. \]

### Final Answer

The exact answer in LaTeX is:
\[ 1.96875 \ln(2). \]

The numerical approximation rounded to 10 decimal places is:
\[ 1.3650449219. \]

Output in JSON format:
```json
{"answer": "1.96875 \\ln(2)", "numerical_answer": "1.3650449219"}
```