<think>
Okay, let's see. I need to compute the definite integral from 0 to π/4 of arctan[(1 + tan x)/√2] dx. Hmm, arctangent integrals can be tricky. Maybe I should start by considering a substitution to simplify the expression inside the arctan. Let me think about possible substitutions.

First, let me recall that integrating arctan of some function might require integration by parts. The standard approach for integrals involving arctan(u) is to let u be the arctan part and dv be dx. Then du would be the derivative of arctan(u) times the derivative of u, and v would be x. But maybe that's not the most straightforward here. Let me write down the integral:

I = ∫₀^{π/4} arctan[(1 + tan x)/√2] dx

Let me denote the argument inside the arctan as a function. Let’s set:

θ(x) = (1 + tan x)/√2

So, I = ∫₀^{π/4} arctan(θ(x)) dx

If I use integration by parts, let u = arctan(θ(x)), dv = dx. Then du = [1/(1 + θ(x)^2)] * θ’(x) dx, and v = x. But integrating by parts would give:

I = x * arctan(θ(x)) | from 0 to π/4 - ∫₀^{π/4} x * [θ’(x)/(1 + θ(x)^2)] dx

Hmm, not sure if that helps. The resulting integral might be more complicated. Maybe there's a substitution that can simplify θ(x). Let me see if there's a trigonometric identity that can help here.

The expression (1 + tan x)/√2. Let me compute tan x in terms of sine and cosine:

tan x = sin x / cos x, so (1 + sin x / cos x)/√2 = (cos x + sin x)/(√2 cos x)

Wait, the numerator is cos x + sin x. That's equal to √2 sin(x + π/4), right? Because sin(a + b) = sin a cos b + cos a sin b. So, √2 sin(x + π/4) = √2 [sin x cos(π/4) + cos x sin(π/4)] = √2 [sin x*(√2/2) + cos x*(√2/2)] = sin x + cos x. So, cos x + sin x = √2 sin(x + π/4). Therefore, the numerator is √2 sin(x + π/4), so:

(1 + tan x)/√2 = [√2 sin(x + π/4)] / (√2 cos x) = sin(x + π/4)/cos x

So θ(x) = sin(x + π/4)/cos x

Hmm, maybe that's helpful. Let me write that:

θ(x) = sin(x + π/4)/cos x

So arctan(θ(x)) = arctan[sin(x + π/4)/cos x]

But sin(x + π/4)/cos x. Let me see if that can be expressed as tan of something. Let's note that sin(x + π/4) = sin x cos(π/4) + cos x sin(π/4) = (sin x + cos x)/√2. Wait, but we already did that. Maybe there's a substitution here. Let me think.

Alternatively, perhaps consider substituting t = x + π/4, but not sure. Alternatively, maybe a substitution that would relate x to another angle such that the argument inside arctan simplifies. Let me think of substitution y = π/4 - x. Let's try that. Let y = π/4 - x. Then when x = 0, y = π/4, and when x = π/4, y = 0. The integral becomes dy = -dx, so the integral I becomes:

I = ∫_{π/4}^0 arctan[(1 + tan(π/4 - y))/√2] (-dy) = ∫₀^{π/4} arctan[(1 + tan(π/4 - y))/√2] dy

So, maybe this substitution can lead to a relation between I and another integral. Let's compute tan(π/4 - y). Using the identity tan(A - B) = (tan A - tan B)/(1 + tan A tan B). So tan(π/4 - y) = [1 - tan y]/[1 + tan y]

Therefore, 1 + tan(π/4 - y) = 1 + [1 - tan y]/[1 + tan y] = [ (1 + tan y) + 1 - tan y ] / (1 + tan y) ) = [2]/(1 + tan y)

So, (1 + tan(π/4 - y))/√2 = [2/(1 + tan y)] / √2 = √2 / (1 + tan y)

Therefore, arctan[√2 / (1 + tan y)]

So, the integral becomes:

I = ∫₀^{π/4} arctan[√2 / (1 + tan y)] dy

But note that arctan(a) + arctan(1/a) = π/2 when a > 0. So, arctan(√2 / (1 + tan y)) = π/2 - arctan[(1 + tan y)/√2]

Therefore, substituting back into the integral:

I = ∫₀^{π/4} [π/2 - arctan((1 + tan y)/√2)] dy = ∫₀^{π/4} π/2 dy - ∫₀^{π/4} arctan((1 + tan y)/√2) dy

But the second integral is the same as the original integral I, but with variable y instead of x. So:

I = (π/2)(π/4) - I

Therefore, I + I = π²/8 => 2I = π²/8 => I = π²/16

Wait, that seems too straightforward. Let me check this step by step.

We let y = π/4 - x, which transformed the original integral into an integral of arctan[√2/(1 + tan y)] dy from 0 to π/4. Then, using the identity arctan(a) + arctan(1/a) = π/2 for a > 0, which is valid here because √2/(1 + tan y) is positive in the interval [0, π/4], since tan y is between 0 and 1. Therefore, arctan(√2/(1 + tan y)) = π/2 - arctan((1 + tan y)/√2). Therefore, substituting back into the integral:

I = ∫₀^{π/4} [π/2 - arctan((1 + tan y)/√2)] dy

But the integral is over y from 0 to π/4, and the integrand is π/2 minus the same function as the original integrand but in terms of y. Therefore, the integral becomes:

I = (π/2)(π/4) - ∫₀^{π/4} arctan((1 + tan y)/√2) dy

But the second term is just the original integral I, since y is a dummy variable. Therefore:

I = π²/8 - I

Then, adding I to both sides:

2I = π²/8 => I = π²/16

So, the exact value of the integral is π squared over 16. That's a neat result! Let me verify this with a numerical approximation to check.

First, compute π²/16. Let's approximate π ≈ 3.1415926536, so π² ≈ 9.8696044011, divided by 16 gives approximately 0.6168502751. Let me compute the integral numerically to check.

Alternatively, let me compute the integral numerically using another method. Let's take x from 0 to π/4, and approximate the integral. Let's pick a few points. But maybe using substitution. Alternatively, since the answer is π²/16, which is approximately 0.6168502751. Let me check with a calculator.

Alternatively, use numerical integration. Let me compute the integral ∫₀^{π/4} arctan[(1 + tan x)/√2] dx numerically. Let me compute this using a numerical method. Let's approximate the integral.

First, let's compute the integral from 0 to π/4 of arctan[(1 + tan x)/√2] dx.

Let me use substitution. Let’s take x from 0 to π/4. Let’s compute the value numerically. Let's use the midpoint rule with a few intervals for approximation. But maybe better to use a calculator.

Alternatively, use the exact result π²/16 ≈ (3.1415926536)^2 /16 ≈ 9.8696044011 /16 ≈ 0.61685027506. So approximately 0.6168502751.

Alternatively, let me check with Wolfram Alpha or a calculator. But since I can't access external resources, I need to trust the analytical steps. The substitution seems valid. The key step was using the substitution y = π/4 - x and then recognizing the identity for arctan(a) + arctan(1/a) = π/2. That led to an equation where I = π²/8 - I, hence 2I = π²/8, so I = π²/16. That seems correct.

Therefore, the exact answer is π²/16, and the numerical approximation is approximately 0.6168502751.
</think>

{"answer": "\\frac{\\pi^2}{16}", "numerical_answer": 0.6168502751}