
To solve the definite integral \(\int_0^1 (x^6 + x^4 + x^2) \cdot \sqrt{2x^4 + 3x^2 + 6} \, dx\), we proceed as follows:


### Step 1: Identify a suitable substitution or antiderivative
The integrand is \((x^6 + x^4 + x^2) \cdot \sqrt{2x^4 + 3x^2 + 6}\). We hypothesize that the integrand is the derivative of a product of a polynomial \(P(x)\) and \(\sqrt{2x^4 + 3x^2 + 6}\). Let \(v = 2x^4 + 3x^2 + 6\), so \(\sqrt{v}\) is the square root term. We assume \(P(x)\) is a polynomial of the form \(P(x) = ax^7 + bx^5 + cx^3\) and use the product rule to match coefficients.


### Step 2: Determine \(P(x)\) by matching coefficients
The derivative of \(P(x) \cdot \sqrt{v}\) is:
\[
\frac{d}{dx} \left[ P(x) \cdot \sqrt{v} \right] = P'(x) \cdot \sqrt{v} + P(x) \cdot \frac{v'}{2\sqrt{v}}
\]
We equate this to the integrand \((x^6 + x^4 + x^2) \cdot \sqrt{v}\). By expanding and matching coefficients of like powers of \(x\), we find:
- \(a = \frac{1}{9}\), \(b = \frac{1}{6}\), \(c = \frac{1}{3}\)

Thus, \(P(x) = \frac{1}{9}x^7 + \frac{1}{6}x^5 + \frac{1}{3}x^3\).


### Step 3: Evaluate the definite integral
The integral is the antiderivative evaluated from \(0\) to \(1\):
\[
\left. P(x) \cdot \sqrt{2x^4 + 3x^2 + 6} \right|_0^1
\]

- At \(x = 1\): \(v(1) = 2(1)^4 + 3(1)^2 + 6 = 11\), so \(\sqrt{v(1)} = \sqrt{11}\).  
  \(P(1) = \frac{1}{9}(1)^7 + \frac{1}{6}(1)^5 + \frac{1}{3}(1)^3 = \frac{1}{9} + \frac{1}{6} + \frac{1}{3} = \frac{11}{18}\).  
  Thus, \(P(1) \cdot \sqrt{v(1)} = \frac{11}{18} \sqrt{11}\).

- At \(x = 0\): \(v(0) = 6\), but \(P(0) = 0\) (since \(P(x)\) has only odd powers of \(x\)). Thus, \(P(0) \cdot \sqrt{v(0)} = 0\).


### Step 4: Final result
The integral evaluates to \(\frac{11}{18} \sqrt{11}\).


### Numerical Approximation
\(\sqrt{11} \approx 3.31662479036\), so:
\[
\frac{11}{18} \sqrt{11} \approx \frac{11 \cdot 3.31662479036}{18} \approx 2.0268262608
\]


{"answer": "\\frac{11\\sqrt{11}}{18}", "numerical_answer": "2.0268262608"}