<think>
Okay, let's see. I need to compute the definite integral from -1 to 0 of 5 times (x^6 + x) to the fourth power dx. Hmm, that looks a bit complicated, but maybe I can expand the expression inside the integral first. 

So, the integrand is 5*(x^6 + x)^4. Expanding (x^6 + x)^4 might be tedious, but perhaps there's a smarter way. Wait, maybe substitution? Let me check if the derivative of the inner function is present. The inner function is u = x^6 + x. The derivative du/dx would be 6x^5 + 1. Hmm, but the integrand is 5*(u)^4, and the derivative here is 6x^5 +1, which doesn't seem to directly multiply into the integrand. So substitution might not work here because the 5 doesn't match with the derivative.

Alternatively, maybe expanding the binomial (x^6 + x)^4. Let's try that. The binomial expansion of (a + b)^4 is a^4 + 4a^3b + 6a^2b^2 + 4ab^3 + b^4. So applying that here:

(x^6 + x)^4 = x^6^4 + 4x^6^3*x + 6x^6^2*x^2 + 4x^6*x^3 + x^4.

Wait, let me compute each term properly. Let's denote a = x^6 and b = x. Then:

(a + b)^4 = a^4 + 4a^3b + 6a^2b^2 + 4ab^3 + b^4.

So substituting back:

First term: a^4 = (x^6)^4 = x^{24}

Second term: 4a^3b = 4*(x^6)^3*x = 4x^{18}* = 4x^{19}

Third term: 6a^2b^2 = 6*(x^6)^2*x^2 = 6x^{12}*x^2 = 6x^{14}

Fourth term: 4ab^3 = 4*x^6*(x)^3 = 4x^{9}

Fifth term: b^4 = x^4

So putting it all together:

(x^6 + x)^4 = x^{24} + 4x^{19} + 6x^{14} + 4x^9 + x^4

Then multiply by 5:

5*(x^{24} + 4x^{19} + 6x^{14} + 4x^9 + x^4) = 5x^{24} + 20x^{19} + 30x^{14} + 20x^9 + 5x^4

Now, the integral becomes the integral from -1 to 0 of each term:

∫_{-1}^0 [5x^{24} + 20x^{19} + 30x^{14} + 20x^9 + 5x^4] dx

We can integrate term by term. Let's compute each integral separately.

First term: ∫5x^{24} dx = 5*(x^{25}/25) = (5/25)x^{25} = (1/5)x^{25}

Second term: ∫20x^{19} dx = 20*(x^{20}/20) = x^{20}

Third term: ∫30x^{14} dx = 30*(x^{15}/15) = 2x^{15}

Fourth term: ∫20x^9 dx = 20*(x^{10}/10) = 2x^{10}

Fifth term: ∫5x^4 dx = 5*(x^5/5) = x^5

So combining all the antiderivatives:

F(x) = (1/5)x^{25} + x^{20} + 2x^{15} + 2x^{10} + x^5

Now, evaluate F(0) - F(-1). Let's compute F(0) first. Plugging in x=0:

All terms have x raised to a positive power, so F(0) = 0.

Now compute F(-1):

Each term:

(1/5)*(-1)^{25} + (-1)^{20} + 2*(-1)^{15} + 2*(-1)^{10} + (-1)^5

Compute each exponent:

(-1)^{25} = -1 (since 25 is odd)

(-1)^{20} = 1 (even)

(-1)^{15} = -1

(-1)^{10} = 1

(-1)^5 = -1

So substituting:

(1/5)*(-1) + 1 + 2*(-1) + 2*(1) + (-1)

Calculate each term:

-1/5) + 1 - 2 + 2 -1

Combine terms:

-0.2 +1 = 0.8

0.8 -2 = -1.2

-1.2 +2 = 0.8

0.8 -1 = -0.2

So F(-1) = -0.2

Therefore, the integral is F(0) - F(-1) = 0 - (-0.2) = 0.2

Wait, 0.2 is 1/5. So the exact answer is 1/5. Let me check that again.

Wait, let's recheck the calculation step by step.

F(-1) = (1/5)(-1)^25 + (-1)^20 + 2*(-1)^15 + 2*(-1)^10 + (-1)^5

Calculating each term:

(1/5)(-1) = -1/5

(-1)^20 = 1

2*(-1)^15 = 2*(-1) = -2

2*(-1)^10 = 2*1 = 2

(-1)^5 = -1

So:

-1/5 +1 -2 +2 -1

Combine:

Start with -1/5 (which is -0.2) +1 = 0.8

0.8 -2 = -1.2

-1.2 +2 = 0.8

0.8 -1 = -0.2

So total F(-1) = -0.2, which is -1/5.

Therefore, the integral is F(0) - F(-1) = 0 - (-1/5) = 1/5.

So the exact answer is 1/5, which is 0.2. Therefore, the numerical approximation is 0.2, which when rounded to 10 decimal places is 0.2000000000.

Wait, but let me confirm that the antiderivatives are correct. Let's check each term:

For the first term: ∫5x^{24} dx. The integral of x^n is x^{n+1}/(n+1). So 5 * x^{25}/25 = x^{25}/5. Correct.

Second term: 20x^{19} integrated is 20 * x^{20}/20 = x^{20}. Correct.

Third term: 30x^{14} integrated is 30 * x^{15}/15 = 2x^{15}. Correct.

Fourth term: 20x^9 integrated is 20 * x^{10}/10 = 2x^{10}. Correct.

Fifth term: 5x^4 integrated is 5 * x^5/5 = x^5. Correct.

So the antiderivative is correct. Then evaluating at 0 gives 0. At -1, as we did, gives -1/5. So the integral is 1/5. That seems surprisingly simple. Let me check if there's a smarter substitution that could have led to this result without expanding.

Wait, maybe there's a substitution. Let me think. Let u = x^5. Then du = 5x^4 dx. Hmm, but the integrand is (x^6 + x)^4. Let's see. If u = x^5, then x^6 = x*u. So x^6 + x = x*u + x = x(u +1). But not sure if that helps. Alternatively, maybe u = x^5 +1? Wait, not sure.

Alternatively, notice that x^6 + x = x(x^5 +1). So (x^6 +x)^4 = x^4(x^5 +1)^4. Then the integrand becomes 5x^4(x^5 +1)^4. Now, that's interesting. Let me see. Let u = x^5 +1. Then du/dx = 5x^4. So 5x^4 dx = du. Therefore, the integral becomes ∫5x^4(x^5 +1)^4 dx = ∫u^4 du. But wait, the original integral is from x=-1 to 0. Let's check the substitution.

If u = x^5 +1, then when x = -1, u = (-1)^5 +1 = -1 +1 = 0. When x=0, u=0^5 +1=1. So the limits of integration become from u=0 to u=1. Therefore, the integral is ∫_{u=0}^{u=1} u^4 du. Which is [u^5 /5] from 0 to1, which is (1/5 -0) =1/5. So that's a much simpler way! So the exact answer is indeed 1/5. So the previous expansion method was correct, but this substitution method is much more straightforward. 

So the integral is 1/5, which is 0.2. Therefore, the numerical approximation is 0.2000000000. So the exact answer is \boxed{\dfrac{1}{5}} and the numerical is 0.2000000000.
</think>

{"answer": "\\dfrac{1}{5}", "numerical_answer": 0.2000000000}