To solve the definite integral \(\int\limits_{0}^{1} x^{-1/2} \left[1 - \sqrt{x(1-x)}\right]^{-5/2} \, dx\), we proceed as follows:

1. **Substitution**: Let \( t = \sqrt{x} \), so \( x = t^2 \) and \( dx = 2t \, dt \). The integral becomes:
   \[
   2 \int_{0}^{1} \left[1 - t \sqrt{1 - t^2}\right]^{-5/2} \, dt
   \]

2. **Second Substitution**: Let \( t = \sin\theta \), so \( dt = \cos\theta \, d\theta \). The integral transforms to:
   \[
   2 \int_{0}^{\pi/2} \left[1 - \sin\theta \cos\theta\right]^{-5/2} \cos\theta \, d\theta
   \]

3. **Further Substitution**: Let \( \phi = 2\theta \), so \( d\phi = 2 \, d\theta \). The integral becomes:
   \[
   \int_{0}^{\pi} \left[1 - \frac{\sin\phi}{2}\right]^{-5/2} \cos\left(\frac{\phi}{2}\right) \, d\phi
   \]

4. **Third Substitution**: Let \( z = \sqrt{\frac{x}{1-x}} \), leading to \( x = \frac{z^2}{1+z^2} \) and \( dx = \frac{2z}{(1+z^2)^2} \, dz \). The integral simplifies to:
   \[
   2 \int_{0}^{\infty} \frac{1+z^2}{(z^2 - z + 1)^{5/2}} \, dz
   \]

5. **Completing the Square**: The denominator \( z^2 - z + 1 \) is rewritten as \( \left(z - \frac{1}{2}\right)^2 + \frac{3}{4} \). Substituting \( u = z - \frac{1}{2} \), the integral splits into two parts which are evaluated separately.

6. **Evaluating the Integrals**:
   - The first integral evaluates to 2.
   - The second integral evaluates to \( \frac{4}{3} \).

7. **Combining Results**: The total integral is:
   \[
   2 \left( 2 + \frac{4}{3} \right) = \frac{20}{3}
   \]

The numerical approximation of \(\frac{20}{3}\) rounded to 10 decimal places is \(6.6666666667\).

### Final Answer
{"answer": "\\dfrac{20}{3}", "numerical_answer": "6.6666666667"}