We wish to evaluate

  I = ∫₀¹ x³·arccos(x)·[arcsin(x)]² dx.

A useful idea is to use the identity

  arccos(x) + arcsin(x) = π/2  for x in [0,1].

Thus we may write

  arccos x = π/2 – arcsin x.

Then the integrand becomes

  x³ [π/2 – arcsin x][arcsin x]² = (π/2)x³(arcsin x)² – x³(arcsin x)³.

In other words, we may write

  I = (π/2)·I₁ – I₂,
  where
    I₁ = ∫₀¹ x³ (arcsin x)² dx  and I₂ = ∫₀¹ x³ (arcsin x)³ dx.

A good change of variable is t = arcsin x so that
  x = sin t  and dx = cos t dt.
When x goes from 0 to 1, t goes from 0 to π/2. Also, note that
  x³ = sin³t.

Thus we have

  I₁ = ∫₀^(π/2) sin³t · t² · cos t dt  and I₂ = ∫₀^(π/2) sin³t · t³ · cos t dt.

A very useful observation is that the factor sin³t cos t dt is the differential of (sin⁴t)/4 because

  d(sin⁴t)/dt = 4 sin³t cos t.

In particular,
  ∫ sin³t cos t dt = sin⁴t/4.

This suggests that we can integrate by parts. We now describe the steps in detail.

Step 1. Write the integrals in a form for integration by parts.
 Define for n = 2,3:
  J(n) = ∫₀^(π/2) tⁿ sin³t cos t dt.
Then we have
  I₁ = J(2) and I₂ = J(3).

Step 2. Integrate by parts in J(n). Write
  u = tⁿ  ⇒ du = n t^(n–1) dt,
  dv = sin³t cos t dt  ⇒ v = sin⁴t/4.
Thus
  J(n) = [tⁿ·(sin⁴t/4)]₀^(π/2) – ∫₀^(π/2) (sin⁴t/4) · n t^(n–1) dt.
For t = π/2 note that sin(π/2)= 1 so sin⁴(π/2)=1, while at 0 the term vanishes. Hence,
  J(n) = ( (π/2)ⁿ / 4 ) – (n/4) L(n–1),
where we have defined
  L(n–1) = ∫₀^(π/2) t^(n–1) sin⁴t dt.

Step 3. In our case we need J(2) and J(3). Thus,
  I₁ = J(2) = ( (π/2)² / 4 ) – (2/4) L(1) = π²/16 – (1/2)L(1),
  I₂ = J(3) = ( (π/2)³ / 4 ) – (3/4) L(2) = π³/32 – (3/4)L(2).

Step 4. We now need to compute L(1) and L(2) where
  L(1) = ∫₀^(π/2) t sin⁴t dt  and L(2) = ∫₀^(π/2) t² sin⁴t dt.
A standard antiderivative (which you can verify using power‐reduction formulas) is
  ∫ sin⁴t dt = (3t/8) – (sin2t/4) + (sin4t/32) + C.
Using integration by parts for L(1) (choosing u = t and dv = sin⁴t dt) one obtains
  L(1) = (3π²/64) + 1/4.
Similarly, an integration by parts for L(2) yields
  L(2) = (2π³ + 17π)/128.
(The details, while straightforward, involve standard techniques and are omitted for brevity.)

Step 5. Substitute back to find I₁ and I₂.
We have
 I₁ = π²/16 – (1/2)[(3π²/64) + 1/4] = π²/16 – (3π²/128) – 1/8.
Writing π²/16 as 8π²/128 this becomes
  I₁ = (8π² – 3π²)/128 – 1/8 = (5π²/128) – 1/8.
Also,
 I₂ = π³/32 – (3/4)[(2π³ + 17π)/128] = π³/32 – (6π³ + 51π)/(512).
Writing π³/32 as 16π³/512 we find
  I₂ = (16π³ – 6π³ – 51π)/512 = (10π³ – 51π)/512.

Step 6. Recall that the original integral is
  I = (π/2)I₁ – I₂.
Substitute I₁ and I₂:
 (π/2)I₁ = π/2 · [(5π²/128) – 1/8] = 5π³/256 – π/16.
Thus,
  I = [5π³/256 – π/16] – [(10π³ – 51π)/512].
To combine these, write the first term with denominator 512:
 5π³/256 = 10π³/512 and π/16 = 32π/512,
so
  I = (10π³/512 – 32π/512) – (10π³/512 – 51π/512)
    = (10π³ – 32π – 10π³ + 51π)/512
    = (19π)/512.

Thus the exact answer is

  I = 19π/512.

Step 7. Numerical approximation.
We have
  π ≈ 3.141592653589793,
so
  I ≈ 19·3.141592653589793/512 ≈ 59.6902604/512 ≈ 0.1166400391.
Rounded to 10 decimal places, this is 0.1166400391.

The final answer in the requested JSON format is:
{"answer": "$\\frac{19\\pi}{512}$", "numerical_answer": "0.1166400391"}