<think>
Okay, so I need to compute the definite integral from 1/√2 to 1 of arcsin(x) divided by x cubed dx. Hmm, let's see. The integral is ∫_{1/√2}^1 [arcsin(x)/x³] dx. Alright, first step is to figure out how to approach this analytically. The integrand has both arcsin(x) and a rational function, so maybe integration by parts would work here. 

Integration by parts formula is ∫u dv = uv - ∫v du. Let me choose u and dv. Since arcsin(x) is a function that can be differentiated, maybe set u = arcsin(x) and dv = 1/x³ dx. Then du would be the derivative of arcsin(x) dx, which is 1/√(1 - x²) dx. And integrating dv would give v. Let's compute v: the integral of 1/x³ is ∫x^(-3) dx = (-1)/(2x²) + C. So v = -1/(2x²).

Applying integration by parts: uv evaluated from 1/√2 to 1 minus ∫v du. So that's [-arcsin(x)/(2x²)] from 1/√2 to 1 minus ∫ [-1/(2x²)] * [1/√(1 - x²)] dx. Let's simplify this. The first term is the evaluation of -arcsin(x)/(2x²) at the limits. Then the integral becomes + (1/2) ∫ [1/(x²√(1 - x²))] dx. 

Now, let's compute the boundary terms first. At x = 1, arcsin(1) is π/2, and 1² is 1, so the term is -π/(2*2*1) = -π/4. At x = 1/√2, arcsin(1/√2) is π/4, and x² is 1/2, so the term is - (π/4)/(2*(1/2)) = - (π/4)/(1) = -π/4. So subtracting these: [-π/4 - (-π/4)] = 0. Wait, that's interesting. The boundary terms cancel out? Wait, no. Wait, the first term is [ -arcsin(1)/(2*1²) ] - [ -arcsin(1/√2)/(2*(1/√2)²) ]. Let me recalculate that.

Wait, the evaluation is upper limit minus lower limit. So:

At upper limit x=1: -arcsin(1)/(2*(1)^2) = - (π/2)/2 = -π/4.

At lower limit x=1/√2: -arcsin(1/√2)/(2*(1/√2)^2) = - (π/4)/(2*(1/2)) = - (π/4)/1 = -π/4.

So the boundary term is (-π/4) - (-π/4) = 0. So the first part cancels out. So the integral reduces to (1/2) ∫ [1/(x²√(1 - x²))] dx from 1/√2 to 1. Now, we need to compute this remaining integral.

Hmm, the integral of 1/(x²√(1 - x²)) dx. Let me think about substitution. Maybe substitute t = x, but not sure. Let's try substitution. Let me set t = sqrt(1 - x²). Then dt/dx = (-x)/sqrt(1 - x²). Hmm, not sure. Alternatively, maybe trigonometric substitution. Since we have sqrt(1 - x²), let's set x = sinθ. Then sqrt(1 - x²) becomes cosθ, and θ = arcsin(x). Let's try that.

Let x = sinθ, so dx = cosθ dθ. Then the integral becomes:

∫ [1/(sin²θ * cosθ)] * cosθ dθ = ∫ 1/sin²θ dθ = ∫ csc²θ dθ = -cotθ + C. So integrating gives -cotθ. Then substituting back θ = arcsin(x), so cotθ = cosθ/sinθ. Since x = sinθ, cosθ = sqrt(1 - x²), so cotθ = sqrt(1 - x²)/x. Therefore, the integral becomes -sqrt(1 - x²)/x + C.

So putting it all together, the remaining integral (1/2) ∫ [1/(x²√(1 - x²))] dx from 1/√2 to 1 is (1/2)[ -sqrt(1 - x²)/x ] evaluated from 1/√2 to 1.

Let's compute that. At x=1: -sqrt(1 - 1)/1 = 0. At x=1/√2: -sqrt(1 - (1/2))/(1/√2) = -sqrt(1/2)/(1/√2) = - (√(1/2)) / (1/√2) = - ( (1/√2) ) / (1/√2) ) = -1. So the integral is (1/2)[0 - (-1)] = (1/2)(1) = 1/2.

Therefore, the entire original integral by parts gives 0 + 1/2 = 1/2. Wait, so the integral is 1/2? Let me check again.

Wait, the integral after integration by parts was (1/2) times the integral of 1/(x²√(1 - x²)) dx. Then we found that integral to be -sqrt(1 - x²)/x evaluated from 1/√2 to 1, which is [0 - (-1)] = 1. Then (1/2)*1 = 1/2. So the entire definite integral is 1/2. Hmm, that seems straightforward, but let me verify.

Wait, but let's check with numerical approximation. Let's compute the integral numerically to see if it's approximately 0.5. Let's take x from 1/√2 ≈0.7071 to 1. The integrand is arcsin(x)/x³. Let's approximate the integral numerically. For example, using trapezoidal rule or Simpson's rule. But maybe just use a calculator. Alternatively, since we have the analytical result as 1/2, but let's check.

Alternatively, let's check the steps again. Integration by parts: u = arcsin(x), dv = x^{-3} dx. Then du = 1/sqrt(1 - x²) dx, v = -1/(2x²). Then the integral is uv| - ∫v du. So uv evaluated from 1/√2 to 1 is [ -arcsin(1)/(2x1²) + arcsin(1/√2)/(2*(1/√2)^2) ].

Wait, arcsin(1) is π/2, so first term is -π/2*1² * 1/2? Wait, no. Wait, uv is u*v. So at x=1, u=π/2, v= -1/(2*1²) = -1/2. So uv is (π/2)*(-1/2) = -π/4. At x=1/√2, u=π/4, v= -1/(2*(1/2)) = -1/(1) = -1. So uv is (π/4)*(-1) = -π/4. Then uv evaluated from upper to lower is (-π/4) - (-π/4) = 0. So that part is correct.

Then the integral becomes 0 - ∫v du. But wait, the formula is uv - ∫v du. So the integral is uv| - ∫v du. But since uv| is 0, then the integral is - ∫v du. But v is -1/(2x²), du is 1/sqrt(1 - x²) dx. So - ∫ (-1/(2x²)) * (1/sqrt(1 - x²)) dx = (1/2) ∫ [1/(x² sqrt(1 - x²))] dx. Then we did substitution x = sinθ, which led to the integral being -sqrt(1 - x²)/x. Evaluated from 1/√2 to 1 gives 0 - (-1) = 1. Then (1/2)*1 = 1/2. So the integral is 1/2. So the exact answer is 1/2. Numerically, 0.5. So that's the result.

Wait, but let me check with a substitution. Let me compute the integral ∫ [arcsin(x)/x³] dx from 1/√2 to 1. If the answer is 1/2, then the numerical approximation should be 0.5. Let me check with a quick numerical estimate. Let's take x=1, the integrand is arcsin(1)/1³ = π/2 ≈1.5708. At x=1/√2≈0.7071, arcsin(0.7071)=π/4≈0.7854, divided by (0.7071)^3≈0.3535, so the integrand is ≈0.7854/0.3535≈2.222. So the function is decreasing from ~2.222 to ~1.5708 over the interval from 0.7071 to 1. The average value might be around (2.222 +1.5708)/2 ≈1.896, multiplied by the interval length (1 - 0.7071)≈0.2929. So approximate integral ≈1.896 *0.2929≈0.555. But according to our analytical result, it's 0.5. Hmm, there's a discrepancy here. So maybe I made a mistake in the analytical solution.

Wait, that's a problem. The numerical estimate here gives around 0.555, but the analytical result is 0.5. So there must be an error in the steps. Let me check again.

Wait, when I did the substitution x = sinθ, let's verify that. The integral after substitution was ∫ [1/(sin²θ * cosθ)] * cosθ dθ. The cosθ cancels, so ∫1/sin²θ dθ = ∫csc²θ dθ = -cotθ + C. Then substituting back θ = arcsin(x), so cotθ = cosθ/sinθ = sqrt(1 - x²)/x. So the integral is -sqrt(1 - x²)/x + C. So when evaluated from 1/√2 to 1:

At x=1: -sqrt(1 -1)/1 = 0.

At x=1/√2: -sqrt(1 - (1/2))/(1/√2) = -sqrt(1/2)/(1/√2) = - (1/√2)/(1/√2) = -1.

So the difference is 0 - (-1) = 1. Then multiplied by 1/2 gives 1/2. So the analytical result is 1/2. But the rough numerical estimate suggested around 0.555. So perhaps my rough estimate was wrong. Let me compute the integral numerically more accurately.

Alternatively, maybe use substitution. Let me compute the integral ∫ [arcsin(x)/x³] dx from a=1/√2 to b=1. Let's use substitution. Let me set t = arcsin(x). Then x = sin t, dx = cos t dt. When x=1/√2, t=π/4. When x=1, t=π/2. The integral becomes ∫_{π/4}^{π/2} [t / sin³ t] * cos t dt = ∫_{π/4}^{π/2} t cos t / sin³ t dt. Let's see if this is easier. Let me write it as ∫ t * cot t * csc² t dt. Hmm, maybe integration by parts again. Let u = t, dv = cot t csc² t dt. Then du = dt. Let's find v. Let me set w = csc t, then dw/dt = -cot t csc t. Hmm, but dv = cot t csc² t dt. Let me see. Let me make substitution for dv: let’s set v’ = cot t csc² t. Let’s let’s set z = csc t, then dz/dt = -cot t csc t. Hmm, but we have cot t csc² t. Let me write it as cot t csc² t = csc t * cot t csc t = csc t * (-dz/dt)). Wait, maybe not. Alternatively, integrate dv = cot t csc² t dt. Let me set u = csc t, then du/dt = -cot t csc t. Hmm, but we have cot t csc² t dt. Let me write it as csc t * cot t csc t dt. Let me set u = csc t, then du = -cot t csc t dt. So then, we have dv = cot t csc² t dt = -csc t * (-cot t csc t dt) = -csc t du. Wait, this is getting complicated. Maybe another substitution. Let me try integrating dv = cot t csc² t dt. Let me set w = csc t, then dw = -cot t csc t dt. So, we have dv = cot t csc² t dt = -w dw. Wait, csc² t = w², and cot t csc t dt = -dw. So cot t csc² t dt = -w * dw. Wait, no. Let me see:

If w = csc t, then dw/dt = -cot t csc t. So, cot t csc t dt = -dw. Then, cot t csc² t dt = cot t csc t * csc t dt = (-dw) * csc t = (-dw) * w. So, dv = -w dw. Therefore, integrating dv gives -w²/2 + C. So v = - (csc² t)/2 + C? Wait, no. Wait, integrating -w dw is - (w²)/2 + C. So v = - (csc² t)/2 + C. Wait, but let's check:

If dv = cot t csc² t dt, and we set w = csc t, then dw = -cot t csc t dt. So, cot t csc² t dt = -csc t dw. But that's not straightforward. Alternatively, maybe integrating by parts again. Let me try integrating dv = cot t csc² t dt. Let me set u = t, dv = cot t csc² t dt. Then du = dt, and v = ?

Wait, integrating dv = cot t csc² t dt. Let me make substitution z = csc t, dz = -cot t csc t dt. Then, cot t csc² t dt = -z dz. So integrating dv gives - (z²)/2 + C = - (csc² t)/2 + C. So v = - (csc² t)/2. Therefore, integration by parts gives uv - ∫v du = t*(-csc² t /2) - ∫ (-csc² t /2) dt. Which is - (t csc² t)/2 + (1/2) ∫ csc² t dt. The integral of csc² t dt is -cot t + C. So putting it all together:

- (t csc² t)/2 + (1/2)(-cot t) + C = - (t csc² t)/2 - (cot t)/2 + C.

Therefore, the integral ∫ t cot t csc² t dt from π/4 to π/2 is [ - (t csc² t)/2 - (cot t)/2 ] evaluated from π/4 to π/2.

At t=π/2: csc(π/2) = 1, cot(π/2)=0. So first term: - (π/2 * 1)/2 - 0 = -π/4. Second term: cot(π/4)=1, csc(π/4)=√2. So at t=π/4: - (π/4 * (√2)^2)/2 - (1)/2 = - (π/4 * 2)/2 - 1/2 = - (π/4) - 1/2. 

So the integral is [ -π/4 ] - [ -π/4 -1/2 ] = (-π/4) + π/4 + 1/2 = 1/2. So the integral from π/4 to π/2 of t cot t csc² t dt is 1/2. Therefore, the original integral is indeed 1/2. So the analytical result is correct. Then my initial rough numerical estimate was wrong. So the exact answer is 1/2, which is 0.5. So the numerical approximation is 0.5. Therefore, the answer is {"answer": "\dfrac{1}{2}", "numerical_answer": 0.5}.
</think>

{"answer": "\\dfrac{1}{2}", "numerical_answer": 0.5000000000}