We start with
  I = ∫₀^(π/4) ln(cot x − 1) dx.

Step 1. Rewrite the integrand in a more convenient form. Note that
  cot x − 1 = (cos x/sin x) − 1 = (cos x − sin x)/sin x.
Thus,
  ln(cot x − 1) = ln(cos x − sin x) − ln(sin x).

Step 2. Express the numerator by factoring out a constant. Observe that
  cos x − sin x = √2 cos(x + π/4)
because cos(x + π/4) = (cos x − sin x)/√2.
Hence,
  ln(cos x − sin x) = ln(√2 cos(x + π/4)) = ln√2 + ln(cos(x + π/4))
             = (½ ln 2) + ln(cos(x + π/4)).

So the integrand becomes:
  ln(cot x − 1) = (½ ln 2) + ln(cos(x + π/4)) − ln(sin x).

Step 3. Write the integral I as:
  I = ∫₀^(π/4) [(½ ln 2) + ln(cos(x + π/4)) − ln(sin x)] dx.
Separate the integral into three parts:
  I = (½ ln 2) ∫₀^(π/4) dx + ∫₀^(π/4) ln(cos(x + π/4)) dx − ∫₀^(π/4) ln(sin x) dx.
The first term is straightforward:
  (½ ln2) ∫₀^(π/4) dx = (½ ln2) · (π/4) = (π/8) ln2.

Step 4. For the second term, perform a substitution:
  Let u = x + π/4, hence du = dx.
When x = 0, u = π/4; when x = π/4, u = π/2.
Thus,
  ∫₀^(π/4) ln(cos(x + π/4)) dx = ∫_(π/4)^(π/2) ln(cos u) du.

Step 5. Recognize a symmetry. Use the substitution v = (π/2) − u in the above integral:
  du = −dv.
When u = π/4, v = π/2 − π/4 = π/4; when u = π/2, v = 0.
Thus, the integral becomes:
  ∫_(π/4)^(π/2) ln(cos u) du = ∫_(π/4)^(0) ln(cos(π/2 − v)) (−dv)
               = ∫₀^(π/4) ln(sin v) dv.
Rename v back to x to obtain:
  ∫_(π/4)^(π/2) ln(cos u) du = ∫₀^(π/4) ln(sin x) dx.

Step 6. Substitute back into I:
  I = (π/8) ln2 + [∫₀^(π/4) ln(sin x) dx] − [∫₀^(π/4) ln(sin x) dx] = (π/8) ln2.
So the entire contribution from the logarithmic integrals cancels out.

Step 7. Thus, the exact answer is:
  I = (π/8) ln2.

Step 8. Numerical approximation:
  π/8 ≈ 0.3926990817 and ln2 ≈ 0.6931471806,
  I ≈ 0.3926990817 × 0.6931471806 ≈ 0.2721982613.

The final answer in the required JSON format is:
{"answer": "\\frac{\\pi}{8}\\ln2", "numerical_answer": "0.2721982613"}