We start with the integral

  I = ∫₁ᵉ x (ln x)² dx.

Step 1. Substitute t = ln x. Then we have:
  x = eᵗ  and  dx = eᵗ dt.
When x = 1, t = ln 1 = 0, and when x = e, t = ln e = 1.
Thus the integral becomes

  I = ∫₀¹ eᵗ (t²)(eᵗ dt) = ∫₀¹ t² e^(2t) dt.

Step 2. To integrate J = ∫ t² e^(2t) dt, use integration by parts.
Let
  u = t²  ⇒ du = 2t dt,
  dv = e^(2t) dt  ⇒ v = e^(2t)/2.
Then
  J = u·v − ∫ v du = (t² e^(2t))/2 − ∫ (e^(2t)/2)(2t dt)
    = (t² e^(2t))/2 − ∫ t e^(2t) dt.

Now, integrate K = ∫ t e^(2t) dt by parts:
Let
  w = t  ⇒ dw = dt,
  dZ = e^(2t) dt  ⇒ Z = e^(2t)/2.
Thus,
  K = w·Z − ∫ Z dw = t·(e^(2t)/2) − ∫ (e^(2t)/2) dt
    = (t e^(2t))/2 − (1/2)[e^(2t)/2]
    = (t e^(2t))/2 − e^(2t)/4
    = e^(2t)(2t − 1)/4.

Returning to J, we have
  J = (t² e^(2t))/2 − K
    = (t² e^(2t))/2 − e^(2t)(2t − 1)/4
    = [2t² e^(2t) − e^(2t)(2t − 1)]/4
    = e^(2t)[2t² − 2t + 1]/4.

Step 3. Evaluate the antiderivative from 0 to 1:
  I = [e^(2t)(2t² − 2t + 1)/4] from t = 0 to 1.
At t = 1:
  e^(2·1) = e²  and 2(1)² − 2(1) + 1 = 2 − 2 + 1 = 1.
At t = 0:
  e^(0) = 1  and 2(0)² − 2(0) + 1 = 1.
Thus,
  I = (1/4)[e²·1 − 1·1] = (e² − 1)/4.

Step 4. Numerical approximation:
  e² ≈ 7.38905609893, so
  (e² − 1)/4 ≈ (7.38905609893 − 1)/4 = 6.38905609893/4 ≈ 1.59726402473.
Rounded to 10 decimal places, the numerical value is 1.5972640247.

{"answer": "\\frac{e^2-1}{4}", "numerical_answer": "1.5972640247"}