Let's compute the integral:
\[
I = \int_0^{\frac{\pi}{2}} x \ln(\sin x)\,dx
\]

**Step 1: Represent \(\ln(\sin x)\) as a series**

Recall the standard Fourier expansion for \(\ln(\sin x)\) for \(0 < x < \pi\):

\[
\ln(\sin x) = -\ln 2 - \sum_{k=1}^{\infty} \frac{\cos(2kx)}{k}
\]

**Step 2: Substitute into the integral**

\[
I = \int_0^{\frac{\pi}{2}} x \ln(\sin x)\,dx = \int_0^{\frac{\pi}{2}} x \left(-\ln 2 - \sum_{k=1}^\infty \frac{\cos(2 k x)}{k}\right) dx
\]
\[
= -\ln 2 \int_0^{\frac{\pi}{2}} x \, dx - \sum_{k=1}^\infty \frac{1}{k} \int_0^{\frac{\pi}{2}} x \cos(2kx)\,dx
\]

Compute the first integral:

\[
\int_0^{\frac{\pi}{2}} x dx = \left.\frac{x^2}{2}\right|_0^{\frac{\pi}{2}} = \frac{\pi^2}{8}
\]

So the first term is:

\[
-\ln 2 \cdot \frac{\pi^2}{8}
\]

**Step 3: Compute \(\int_0^{\frac{\pi}{2}} x \cos(2kx)\,dx\)**

Letâ€™s compute:
\[
I_k = \int_0^{\frac{\pi}{2}} x \cos(2k x)\,dx
\]

Use integration by parts:

Let \(u = x\), \(dv = \cos(2k x)dx\), so \(du = dx\), \(v = \frac{\sin(2k x)}{2k}\):

\[
I_k = x \cdot \frac{\sin(2k x)}{2k} \Big|_0^{\frac{\pi}{2}} - \int_0^{\frac{\pi}{2}} \frac{\sin(2k x)}{2k}dx
\]
\[
= \frac{\pi}{2} \cdot \frac{\sin(k\pi)}{2k} - 0 - \frac{1}{2k} \int_0^{\frac{\pi}{2}} \sin(2k x) dx
\]

But \(\sin(k\pi) = 0\) for integer \(k\), so:

\[
I_k = - \frac{1}{2k} \int_0^{\frac{\pi}{2}} \sin(2k x) dx
\]
\[
\int_0^{\frac{\pi}{2}} \sin(2k x) dx = \left.\frac{-\cos(2k x)}{2k}\right|_0^{\frac{\pi}{2}} = \frac{-\cos(k\pi) + 1}{2k}
\]
Recall: \(\cos(k\pi) = (-1)^k\)

So:
\[
I_k = -\frac{1}{2k} \cdot \frac{-(-1)^k + 1}{2k} = \frac{1 - (-1)^k}{4k^2}
\]

**Step 4: Substitute back**

Thus,

\[
I = -\ln 2 \cdot \frac{\pi^2}{8} - \sum_{k=1}^\infty \frac{1}{k} \cdot \frac{1 - (-1)^k}{4k^2}
\]
\[
= -\ln 2 \cdot \frac{\pi^2}{8} - \sum_{k=1}^\infty \frac{1 - (-1)^k}{4k^3}
\]

Note that \(1 - (-1)^k\) is zero for even \(k\), and \(2\) for odd \(k\):

For \(k\) odd (\(k = 2n+1\)):
\[
1 - (-1)^k = 1 - (-1)^{2n+1} = 1 - (-1) = 2
\]

So:

\[
\sum_{k=1}^\infty \frac{1 - (-1)^k}{4k^3} = \sum_{n=0}^\infty \frac{2}{4(2n+1)^3} = \frac{1}{2} \sum_{n=0}^\infty \frac{1}{(2n+1)^3}
\]

But,
\[
\sum_{n=0}^\infty \frac{1}{(2n+1)^3} = \sum_{k=1,\,k\,\text{odd}}^\infty \frac{1}{k^3} = \sum_{k=1}^\infty \frac{1}{k^3} - \sum_{k=1}^\infty \frac{1}{(2k)^3}
\]
\[
= \zeta(3) - \frac{1}{8}\zeta(3) = \frac{7}{8} \zeta(3)
\]

Thus,

\[
\frac{1}{2} \sum_{n=0}^\infty \frac{1}{(2n+1)^3} = \frac{1}{2} \cdot \frac{7}{8} \zeta(3) = \frac{7}{16} \zeta(3)
\]

**Final exact result:**

\[
I = -\frac{\pi^2}{8} \ln 2 - \frac{7}{16} \zeta(3)
\]

**Step 5: Numerical Evaluation**

\[
\pi^2 \approx 9.8696044011
\]
\[
\frac{\pi^2}{8} \approx 1.2337005501
\]
\[
\ln 2 \approx 0.6931471806
\]
\[
\frac{\pi^2}{8} \ln 2 \approx 1.2337005501 \times 0.6931471806 \approx 0.8556260872
\]
\[
\zeta(3) \approx 1.2020569032
\]
\[
\frac{7}{16} \zeta(3) = 0.4375 \times 1.2020569032 \approx 0.5258978941
\]
So
\[
I \approx -0.8556260872 - 0.5258978941 = -1.3815239813
\]

**JSON output required:**
```json
{"answer": "-\\frac{\\pi^2}{8}\\ln 2 - \\frac{7}{16}\\zeta(3)", "numerical_answer": "-1.3815239813"}
```