Given:
\[
I = \int_{1}^{\infty} (x^2-1^2)^{2-1/2} e^{-0.5^2 x^2} H_{2\times 2+1}(0.5x) \; dx
\]
Let's clarify each component:
- \(x^2-1^2 = x^2-1\)
- Exponent: \((2-1/2) = 3/2\)
- \(e^{-0.5^2 x^2} = e^{-0.25 x^2}\)
- Hermite polynomial \(H_{2\times 2+1}(0.5x) = H_5(0.5x)\)

So,
\[
I = \int_1^\infty (x^2-1)^{3/2} e^{-0.25 x^2} H_5(0.5x)\; dx
\]

**Step 1: Simplify and Analyze Hermite Polynomial**

The physicists' Hermite polynomial \(H_5(x)\):
\[
H_5(x) = 32x^5 - 160x^3 + 120x
\]
So,
\[
H_5(0.5x) = 32(0.5x)^5 - 160(0.5x)^3 + 120(0.5x) = 32\cdot \frac{x^5}{32} - 160 \cdot \frac{x^3}{8} + 120 \cdot \frac{x}{2}
\]
\[
= x^5 - 20x^3 + 60x
\]

Therefore, the integrand is:
\[
(x^2 - 1)^{3/2} e^{-0.25x^2} (x^5 - 20x^3 + 60x)
\]

**Step 2: Expand the Integral**

Expand \((x^2-1)^{3/2}\):

Let’s let \(u = x^2-1\), so \(du = 2x dx\), but expressing everything in terms of \(x\) is easier given the limits.

So the integrand is:
\[
(x^2-1)^{3/2} e^{-0.25 x^2} x^5 - 20 (x^2-1)^{3/2} e^{-0.25 x^2} x^3 + 60 (x^2-1)^{3/2} e^{-0.25 x^2} x
\]
Thus,
\[
I = \int_1^\infty (x^2-1)^{3/2} e^{-0.25 x^2} [x^5 - 20x^3 + 60x] dx
\]

**Step 3: Substitution**

Let's try a substitution: set \(x = \cosh t\), for \(x \geq 1\) we have \(t \in [0, \infty)\):

Then,
- \(x^2-1 = \cosh^2 t - 1 = \sinh^2 t\)
- \((x^2-1)^{3/2} = (\sinh^2 t)^{3/2} = \sinh^3 t\)
- \(dx = \sinh t dt\)
- \(x = \cosh t\)
- \(x^3 = \cosh^3 t\)
- \(x^5 = \cosh^5 t\)
- \(e^{-0.25 x^2} = e^{-0.25 \cosh^2 t}\)

So the integral becomes (limits: \(x=1 \implies t=0\), \(x\to\infty \implies t\to\infty\)):
\[
I = \int_{t=0}^{\infty} \sinh^3 t\, e^{-0.25 \cosh^2 t} \left[
\cosh^5 t - 20 \cosh^3 t + 60 \cosh t
\right]\sinh t\, dt
\]
\[
= \int_0^\infty \sinh^4 t\, e^{-0.25 \cosh^2 t} \left(\cosh^5 t - 20 \cosh^3 t + 60 \cosh t\right) dt
\]

**Step 4: Further Simplification**

Expand the product:
\[
I = \int_{0}^{\infty} \sinh^4 t\,\cosh^5 t\, e^{-0.25 \cosh^2 t} dt - 20 \int_0^\infty \sinh^4 t\, \cosh^3 t\, e^{-0.25 \cosh^2 t} dt + 60 \int_0^\infty \sinh^4 t\, \cosh t\, e^{-0.25 \cosh^2 t} dt
\]

Let’s write:
\[
I = I_1 - 20 I_2 + 60 I_3
\]
where
\[
I_n = \int_0^\infty \sinh^4 t\, \cosh^n t\, e^{-0.25 \cosh^2 t} dt
\]
for \(n = 5, 3, 1\).

Expand \(\sinh^4 t = (\frac{e^t - e^{-t}}{2})^4\), but that's laborious. Since we're expected to provide an analytical expression but also a precise numerical value, let's seek a more effective approach.

**Step 5: Generalized Expression and Identification**

For the integral:
\[
J_{m, n}(a) = \int_0^\infty \sinh^m t\, \cosh^n t\, e^{-a \cosh^2 t} dt
\]
it is related to parabolic cylinder functions or confluent hypergeometric functions, but closed forms exist for certain values. However, due to the high powers here, a general closed-form is unwieldy.

Given the form, let's instead revert to a substitution in \(x\)-space to attempt a manageable form.

Alternatively, let's try reducing the power:

Since the integrand contains a factor of \((x^2 - 1)^{3/2}\) times a polynomial and a Gaussian, try substituting \(x = r\), \(dx = dr\).

Let’s try the substitutions in the original variable:

- Use \(u = x^2\), then \(x^2 - 1 = u - 1\), \(dx = \frac{du}{2\sqrt{u}}\), \(x = \sqrt{u}\).
- When \(x=1\), \(u=1\).
- When \(x=\infty\), \(u=\infty\).
- The polynomial in \(x\) can be expressed in \(u\).

Let’s expand \(x^5 - 20 x^3 + 60 x\):

- \(x^5 = (x^2)^{2} x = u^2 x\)
- \(x^3 = (x^2) x = u x\)

So,
\[
x^5 - 20x^3 + 60x = x(u^2 - 20u + 60)
\]
But since \(x = \sqrt{u}\), then
\[
x(u^2 - 20u + 60) = \sqrt{u} (u^2 - 20u + 60)
\]

Thus,
\[
I = \int_{x=1}^{\infty} (x^2 - 1)^{3/2} e^{-0.25 x^2} x(u^2 - 20u + 60) dx
\]
Express \(x^2 = u\):

\[
I = \int_{u=1}^{\infty} (u - 1)^{3/2} e^{-0.25 u} \sqrt{u} (u^2 - 20 u + 60) \frac{du}{2\sqrt{u}}
\]
\[
= \frac{1}{2} \int_{1}^{\infty} (u - 1)^{3/2} e^{-0.25 u} (u^2 - 20u + 60) du
\]

**Step 6: Final Analytical Expression**

So, the integral simplifies to:
\[
I = \frac{1}{2} \int_{1}^{\infty} (u-1)^{3/2} (u^2 - 20u + 60) e^{-0.25 u} du
\]

This is an exact analytical expression, reducible to sums of incomplete gamma functions, but let's write it in a decomposed sum:

Let \( (u-1)^{3/2} (u^2-20u+60) \) = \( (u-1)^{3/2}u^2 - 20(u-1)^{3/2}u + 60(u-1)^{3/2} \).

Therefore,
\[
I = \frac{1}{2} \left[ \int_{1}^{\infty} (u-1)^{3/2}u^2 e^{-0.25u} du - 20 \int_{1}^{\infty} (u-1)^{3/2}u e^{-0.25u} du + 60 \int_{1}^{\infty} (u-1)^{3/2} e^{-0.25u} du \right]
\]

Let’s define:
\[
J_n = \int_{1}^{\infty} (u-1)^{3/2} u^n e^{-0.25u} du
\]
for \(n=2,1,0\):

So,
\[
I = \frac{1}{2} \left[ J_2 - 20 J_1 + 60 J_0 \right]
\]

The integrals \(J_n\) can be expressed in terms of the upper incomplete gamma function using the substitution \(w=u-1\), \(u = w+1\), \(du=dw\):

- When \(u=1\), \(w=0\)
- When \(u \to \infty\), \(w \to \infty\)

For \(J_n\):
\[
J_n = \int_{w=0}^{\infty} w^{3/2} (w+1)^n e^{-0.25 (w+1)} dw
= e^{-0.25} \int_{0}^{\infty} w^{3/2} (w+1)^n e^{-0.25 w} dw
\]

\((w+1)^n\) can be binomial-expanded:
\[
(w+1)^n = \sum_{k=0}^n \binom{n}{k} w^k
\]
Therefore,
\[
w^{3/2}(w+1)^n = \sum_{k=0}^n \binom{n}{k} w^{k+3/2}
\]
So,
\[
J_n = e^{-0.25} \sum_{k=0}^n \binom{n}{k} \int_0^\infty w^{k+3/2} e^{-0.25 w} dw
\]
\[
= e^{-0.25} \sum_{k=0}^n \binom{n}{k} \Gamma(k+5/2) (0.25)^{-(k+5/2)}
\]

Because
\[
\int_{0}^{\infty} x^{a-1} e^{-\beta x} dx = \beta^{-a} \Gamma(a)
\]
with \(a = k+5/2\), \(\beta = 0.25\).

Therefore,
\[
J_n = e^{-0.25} \cdot 4^{k+5/2} \sum_{k=0}^{n} \binom{n}{k} \Gamma(k+5/2)
\]

But each term is \(e^{-0.25} \binom{n}{k} \cdot \Gamma(k+5/2) \cdot 4^{k+5/2}\).

**Thus:**

\[
J_n = e^{-0.25} \sum_{k=0}^n \binom{n}{k} \Gamma\left(k+\frac{5}{2}\right) 4^{k+5/2}
\]

But  \(0.25^{-(k+5/2)} = 4^{k+5/2}\).

Therefore,
\[
I = \frac{1}{2} \; e^{-0.25} \sum_{n=0}^{2} a_n \sum_{k=0}^{n} \binom{n}{k} \Gamma(k+5/2) 4^{k+5/2}
\]
where the coefficients:
- for \(n=2, a_2=1\)
- for \(n=1, a_1=-20\)
- for \(n=0, a_0=60\)

So:
\[
I = \frac{1}{2} e^{-0.25} \left( S_2 - 20 S_1 + 60 S_0 \right)
\]
where
\[
S_n = \sum_{k=0}^n \binom{n}{k} \Gamma(k+5/2) 4^{k+5/2}
\]

**Explicitly:**

- For \(S_2\):
  - \(k=0\): \(\Gamma(5/2)4^{5/2}\)
  - \(k=1\): \(2\Gamma(7/2)4^{7/2}\)
  - \(k=2\): \(\Gamma(9/2)4^{9/2}\)

- For \(S_1\):
  - \(k=0\): \(\Gamma(5/2)4^{5/2}\)
  - \(k=1\): \(\Gamma(7/2)4^{7/2}\)

- For \(S_0\):
  - \(k=0\): \(\Gamma(5/2)4^{5/2}\)

Explicitly:
\[
S_2 = \Gamma\left(\frac{5}{2}\right) 4^{5/2} + 2\Gamma\left(\frac{7}{2}\right) 4^{7/2} + \Gamma\left(\frac{9}{2}\right) 4^{9/2}
\]
\[
S_1 = \Gamma\left(\frac{5}{2}\right) 4^{5/2} + \Gamma\left(\frac{7}{2}\right) 4^{7/2}
\]
\[
S_0 = \Gamma\left(\frac{5}{2}\right) 4^{5/2}
\]

Now, collect terms for the final analytical answer:

\[
I = \frac{1}{2} e^{-0.25}
\left\{
\left[ \Gamma\left(\frac{5}{2}\right)4^{5/2} + 2\Gamma\left(\frac{7}{2}\right)4^{7/2} + \Gamma\left(\frac{9}{2}\right)4^{9/2}\right]
-20 \left[ \Gamma\left(\frac{5}{2}\right)4^{5/2} + \Gamma\left(\frac{7}{2}\right)4^{7/2} \right]
+60 \Gamma\left(\frac{5}{2}\right)4^{5/2}
\right\}
\]

Or combining:

\[
I = \frac{1}{2} e^{-0.25} \left\{
(1 - 20 + 60) \Gamma\left(\frac{5}{2}\right)4^{5/2}
+ (2 - 20)\Gamma\left(\frac{7}{2}\right)4^{7/2}
+ \Gamma\left(\frac{9}{2}\right)4^{9/2}
\right\}
\]

\[
= \frac{1}{2} e^{-0.25} \left\{
41 \Gamma\left(\frac{5}{2}\right) 4^{5/2}
- 18 \Gamma\left(\frac{7}{2}\right) 4^{7/2}
+ \Gamma\left(\frac{9}{2}\right) 4^{9/2}
\right\}
\]

**Step 7: Substitute Gamma and Compute Numerically**

Recall:
- \(\Gamma\left(\frac{5}{2}\right) = \frac{3\sqrt{\pi}}{4}\)
- \(\Gamma\left(\frac{7}{2}\right) = \frac{15\sqrt{\pi}}{8}\)
- \(\Gamma\left(\frac{9}{2}\right) = \frac{105\sqrt{\pi}}{16}\)

- \(4^{5/2} = 32\)
- \(4^{7/2} = 128\)
- \(4^{9/2} = 512\)

Now substitute:

- \(\Gamma\left(\frac{5}{2}\right) 4^{5/2} = \frac{3\sqrt{\pi}}{4} \cdot 32 = 24\sqrt{\pi}\)
- \(\Gamma\left(\frac{7}{2}\right) 4^{7/2} = \frac{15\sqrt{\pi}}{8} \cdot 128 = 240\sqrt{\pi}\)
- \(\Gamma\left(\frac{9}{2}\right) 4^{9/2} = \frac{105\sqrt{\pi}}{16} \cdot 512 = 3360\sqrt{\pi}\)

So:
\[
I = \frac{1}{2} e^{-0.25} \left(41 \times 24\sqrt{\pi} - 18 \times 240\sqrt{\pi} + 3360\sqrt{\pi}\right)
\]
\[
= \frac{1}{2} e^{-0.25} \left(984\sqrt{\pi} - 4320\sqrt{\pi} + 3360\sqrt{\pi}\right)
\]
\[
= \frac{1}{2} e^{-0.25} \left((984 + 3360 - 4320) \sqrt{\pi}\right)
\]
\[
= \frac{1}{2} e^{-0.25} (24\sqrt{\pi})
\]
\[
= 12 \sqrt{\pi} e^{-0.25}
\]

**Step 8: Numerical Evaluation**

- \(e^{-0.25} \approx 0.7788007831\)
- \(\sqrt{\pi} \approx 1.7724538509\)

Thus:
\[
12 \cdot 1.7724538509 \cdot 0.7788007831 \approx 12 \cdot 1.3793629642 \approx 16.5523555704
\]

**Step 9: Final JSON Output**

```json
{"answer": "12 \\sqrt{\\pi} e^{-0.25}", "numerical_answer": "16.5523555704"}
```