We wish to evaluate

  I = ∫₁∞ (x² – 1)^(2 – ½) exp[–(0.5)² x²] H₍₂×2+1₎(0.5x) dx.

Step 1. Write the Integral in a Simplified Form

Notice that
  2 – ½ = 3/2   and  2×2+1 = 5.
Also, (0.5)² = 0.25. Thus the integral becomes

  I = ∫₁∞ (x² – 1)^(3/2) e^(–x²/4) H₅(0.5x) dx.

For the (physicists’) Hermite polynomials, one has
  H₅(z) = 32z⁵ – 160z³ + 120z.
Hence, with z = 0.5x we obtain

  H₅(0.5x) = 32(0.5x)⁵ – 160(0.5x)³ + 120(0.5x)
          = 32·(x⁵/32) – 160·(x³/8) + 60x
          = x⁵ – 20x³ + 60x.

Thus the integrand becomes

  (x² – 1)^(3/2) e^(–x²/4) (x⁵ – 20x³ + 60x).

So

  I = ∫₁∞ (x² – 1)^(3/2) (x⁵ – 20x³ + 60x) e^(–x²/4) dx.

Step 2. Change of Variables

It is advantageous to remove the “–1” from (x² – 1). Set

  u = x² – 1  ⟹ x = √(u+1),
  du = 2x dx  ⟹ dx = du/(2√(u+1)).

When x = 1, u = 0 and when x → ∞, u → ∞. Also,
  (x² – 1)^(3/2) becomes u^(3/2),
and
  x⁵ – 20x³ + 60x = (√(u+1))⁵ – 20 (√(u+1))³ + 60 √(u+1)
       = (u+1)^(5/2) – 20 (u+1)^(3/2) + 60 (u+1)^(1/2).

Including the factor dx = du/(2√(u+1)), we see that

  [(u+1)^(5/2) – 20 (u+1)^(3/2) + 60 (u+1)^(1/2)] / √(u+1)
     = (u+1)² – 20(u+1) + 60.

A short algebra shows:
  (u+1)² – 20(u+1) + 60 = u² + 2u + 1 – 20u – 20 + 60 = u² – 18u + 41.

Also, the exponential becomes
  e^(–x²/4) = e^(–(u+1)/4) = e^(–1/4)e^(–u/4).

Thus the integral transforms to

  I = ∫₀∞ u^(3/2) e^(–1/4) e^(–u/4) [u² – 18u + 41] · (du/2)
     = (e^(–1/4)/2) ∫₀∞ u^(3/2) (u² – 18u + 41)e^(–u/4) du.

Step 3. Write the Integral as a Combination of Gamma Integrals

Write the polynomial factor explicitly:

  I = (e^(–1/4)/2) { ∫₀∞ u^(3/2 + 2)e^(–u/4) du – 18∫₀∞ u^(3/2+1)e^(–u/4) du + 41∫₀∞ u^(3/2)e^(–u/4) du }.
That is,
  I = (e^(–1/4)/2) [ I₁ – 18 I₂ + 41 I₃ ],
with
  I₁ = ∫₀∞ u^(7/2)e^(–u/4) du,
  I₂ = ∫₀∞ u^(5/2)e^(–u/4) du,
  I₃ = ∫₀∞ u^(3/2)e^(–u/4) du.

Recall the Gamma integral:
  ∫₀∞ u^(p–1)e^(–βu)du = Γ(p)/βᵖ.
For our integrals, write the exponent in the form u^(p–1):
  For I₁, we have 7/2 = p – 1, so p = 9/2.
  For I₂, 5/2 = p – 1, so p = 7/2.
  For I₃, 3/2 = p – 1, so p = 5/2.
Also, β = 1/4 here. Therefore,
  I₁ = Γ(9/2) / (1/4)^(9/2) = Γ(9/2)·4^(9/2),
  I₂ = Γ(7/2)·4^(7/2),
  I₃ = Γ(5/2)·4^(5/2).

Step 4. Evaluate the Gamma Functions and Powers

The needed Gamma values are:
  Γ(9/2) = (7/2)(5/2)(3/2)(1/2)√π = (7·5·3·1 √π)/(2⁴) = 105√π/16,
  Γ(7/2) = (5/2)(3/2)(1/2)√π = 15√π/8,
  Γ(5/2) = (3/2)(1/2)√π = 3√π/4.

Also, note
  4^(9/2) = (√4)^9 = 2^9 = 512,
  4^(7/2) = 2^7 = 128,
  4^(5/2) = 2^5 = 32.

Now substitute:
  I₁ = (105√π/16) · 512 = 105√π · (512/16) = 105√π · 32 = 3360√π,
  I₂ = (15√π/8) · 128 = 15√π · (128/8) = 15√π · 16 = 240√π,
  I₃ = (3√π/4) · 32 = 3√π · (32/4) = 3√π · 8 = 24√π.

Now, plug these back in:

  I = (e^(–1/4)/2)[3360√π – 18·(240√π) + 41·(24√π)]
     = (e^(–1/4)/2)[3360√π – 4320√π + 984√π].

Combine the coefficients:

  3360 – 4320 + 984 = (3360 – 4320) + 984 = (–960) + 984 = 24.

Thus,
  I = (e^(–1/4)/2) · 24√π = 12√π e^(–1/4).

Step 5. Numerical Approximation

We now compute a numerical value. Recall:
  √π ≈ 1.772453850905516,
  e^(–1/4) = e^(–0.25) ≈ 0.778800783071405.
Then

  12√π ≈ 12 × 1.772453850905516 = 21.269446210866192,
  I ≈ 21.269446210866192 × 0.778800783071405 ≈ 16.5612097163.

Rounded to 10 decimal places this is 16.5612097163.

Step 6. Final Answer in JSON Format

{"answer": "12\\\\sqrt{\\\\pi}e^{-\\\\frac{1}{4}}", "numerical_answer": "16.5612097163"}