We wish to evaluate

  I = ∫₀^(∞) [1/(x(x²+1))] · arctan(x/(x²+1)) dx.

Step 1. (Symmetrizing the integral using the substitution x → 1/x)

Make the substitution x = 1/t. Then:
  dx = –dt/t²,
and note that
  x²+1 = (1/t²)+1 = (1+t²)/t²,
so
  1/(x(x²+1)) becomes
    1/[(1/t)·((1+t²)/t²)] = t³/(1+t²),
and also
  arctan(x/(x²+1)) becomes
    arctan[(1/t)/( (1+t²)/t² )] = arctan[t/(1+t²)].
Thus the integral transforms into
  I = ∫_∞^0 { t³/(1+t²) · arctan[t/(1+t²)] · (–1/t²) } dt
    = ∫₀^(∞) { t/(1+t²) · arctan[t/(1+t²)] } dt.
We now have two equivalent representations for I:
  I = ∫₀^(∞) [1/(x(x²+1))] arctan(x/(x²+1)) dx            (1)
  I = ∫₀^(∞) [x/(1+x²)] arctan(x/(1+x²)) dx            (2)

Add the two forms (with the same change of dummy variable) to obtain:
  2I = ∫₀^(∞) { [1/(x(x²+1)) + x/(1+x²)] · arctan(x/(x²+1)) } dx.
Notice that
  1/(x(x²+1)) + x/(1+x²) = (1 + x²)/(x(1+x²)) = 1/x.
Thus,
  2I = ∫₀^(∞) [1/x] · arctan(x/(x²+1)) dx,
or
  I = (1/2) ∫₀^(∞) [1/x] · arctan(x/(x²+1)) dx.          (3)

Step 2. (Change of Variable: t = ln x)

Let u = ln x so that x = eᵘ and dx = eᵘ du. Then 1/x dx = du and the limits become u → –∞ to u → ∞. Also, note that
  x/(x²+1) = eᵘ/(e^(2u)+1).
Multiply numerator and denominator by e^(–u):
  eᵘ/(e^(2u)+1) = 1/(eᵘ + e^(–u)).
But eᵘ + e^(–u) = 2 cosh u, so
  x/(x²+1) = 1/(2 cosh u),
and hence
  arctan(x/(x²+1)) = arctan[1/(2 cosh u)].
Then (3) becomes
  I = (1/2) ∫_(–∞)^(∞) arctan[1/(2 cosh u)] du.
Because the integrand is even in u we have
  ∫_(–∞)^(∞) arctan[1/(2 cosh u)] du = 2 ∫₀^(∞) arctan[1/(2 cosh u)] du.
Thus,
  I = (1/2)·2 ∫₀^(∞) arctan[1/(2 cosh u)] du = ∫₀^(∞) arctan[1/(2 cosh u)] du.   (4)

Step 3. (Introducing a parameter)

Write the integral in the form
  F(a) = ∫₀^(∞) arctan[a/cosh u] du,
so that our desired I is F(1/2).

Differentiate F(a) with respect to a:
  F′(a) = ∫₀^(∞) d/da { arctan(a/cosh u) } du
     = ∫₀^(∞) [1/(1+(a/cosh u)²)] · (1/cosh u) du
     = ∫₀^(∞) cosh u / [cosh² u + a²] du.
Now, substitute t = sinh u so that dt = cosh u du and note cosh² u = 1+t². Then
  F′(a) = ∫₀^(∞) dt/(1+t²+a²) = ∫₀^(∞) dt/(t² + (a²+1)).
This is a standard integral with result
  ∫₀^(∞) dt/(t²+β²) = π/(2β)   (with β = √(a²+1)).
Thus,
  F′(a) = π/(2√(a²+1)).
Integrate with respect to a:
  F(a) = ∫₀^a π/(2√(s²+1)) ds = (π/2) asinh(a),
since ∫ ds/√(s²+1) = asinh(s) and F(0) = 0.

So,
  F(1/2) = (π/2) asinh(1/2).
Recall that asinh(1/2) = ln[1/2 + √(1/4+1)] = ln[(1+√5)/2].

Thus, our result is
  I = (π/2) ln[(1+√5)/2].

Step 4. (Numerical Approximation)

We compute:
  (1+√5)/2 ≈ (1+2.2360679775)/2 ≈ 1.61803398875,
  ln(1.61803398875) ≈ 0.48121182506,
so
  I ≈ (π/2) · 0.48121182506 ≈ 1.57079632679 · 0.48121182506 ≈ 0.7558857670.

Final Answer in JSON:
{"answer": "\\frac{\\pi}{2}\\ln\\frac{1+\\sqrt{5}}{2}", "numerical_answer": "0.7558857670"}