Let's carefully solve the integral:
\[
I = \int_{0}^{1} \arccos x\, \mathbf{D}(0.5x)\, dx
\]
where \(\mathbf{D}(z)\) denotes the **Dawson function**:
\[
\mathbf{D}(z) = e^{-z^2} \int_0^z e^{t^2} dt
\]

### Step 1: Substitution

Let \(u = 0.5x\), so \(x = 2u\), \(dx = 2 du\).

When \(x=0\), \(u=0\). When \(x=1\), \(u=0.5\).

So, the integral becomes:
\[
I = \int_{x=0}^{x=1} \arccos x\ \mathbf{D}(0.5x)\ dx = \int_{u=0}^{u=0.5} \arccos(2u)\, \mathbf{D}(u)\ 2\, du
\]
\[
I = 2 \int_{0}^{0.5} \arccos(2u)\, \mathbf{D}(u)\, du
\]

### Step 2: Integration by Parts

Let:
- \(u_1 = \arccos(2u)\) \(\implies\) \(du_1 = \frac{-2}{\sqrt{1-(2u)^2}} du = \frac{-2}{\sqrt{1-4u^2}} du\)
- \(dv_1 = \mathbf{D}(u) du\) \(\implies\) \(v_1 = \int \mathbf{D}(u) du\)

Recall the derivative: \(\frac{d}{dz}\mathbf{D}(z) = 1 - 2z \mathbf{D}(z)\), so the antiderivative is not elementary. However, let's proceed:

Integration by parts formula:
\[
\int f(x) g'(x) dx = f(x) g(x) - \int f'(x) g(x) dx
\]
but here, better to use the *differentiation under the integral sign* technique.

But first, let's try integrating by parts:
\[
I = 2 \int_{0}^{0.5} \arccos(2u)\, \mathbf{D}(u)\, du
\]

Take:
- \(f(u) = \arccos(2u)\)
- \(dg = \mathbf{D}(u) du\)

Let:
- \(df(u) = \frac{-2}{\sqrt{1-4u^2}} du\)
- \(g(u) = \int \mathbf{D}(u) du\)

But the integral of Dawson's function does not have a simple expression.

#### Try Differentiation Under the Integral Sign

Let’s instead try differentiating under the integral sign or recognize that this integral likely appears in tables or references.

### Step 3: Another Approach— Differentiation with respect to a parameter

Introduce a parameter \(a\) setting \(x = a u\), \(dx = a\, du\), adjusting the limits accordingly:

But since \(0.5x\) just scales the argument of Dawson, and Dawon's function is the odd part of the complex error function, let's consider if the integral can be simplified via known integrals or properties.

But since \(g(u) = \int \mathbf{D}(u) du\) is not elementary, let's try differentiating \(I(\alpha) = \int_0^1 \arccos x\, \mathbf{D}(\alpha x)\, dx\) with respect to \(\alpha\), and set \(\alpha = 0.5\) at the end.

Let:
\[
I(\alpha) = \int_{0}^{1} \arccos x\ \mathbf{D}(\alpha x)\ dx
\]
Then,
\[
\frac{dI}{d\alpha} = \int_{0}^{1} \arccos x\ \frac{d}{d\alpha} \mathbf{D}(\alpha x)\ dx
\]

Since \(\frac{d}{dz}\mathbf{D}(z) = 1 - 2z \mathbf{D}(z)\),
\[
\frac{d}{d\alpha} \mathbf{D}(\alpha x) = x\, \mathbf{D}'(\alpha x) = x (1 - 2 \alpha x \mathbf{D}(\alpha x))
\]

Thus,
\[
\frac{dI}{d\alpha} = \int_{0}^{1} \arccos x\, x\, dx - 2\alpha \int_{0}^{1} \arccos x\, x^2\, \mathbf{D}(\alpha x)\ dx
\]

Now, set \(J_1 = \int_0^1 \arccos x\, x\, dx\).

Let’s compute \(J_1\):

Let \(x = \cos \theta\), so \(dx = -\sin \theta d\theta\).

When \(x=0\), \(\theta = \arccos 0 = \pi/2\); when \(x = 1\), \(\theta = 0\).

So:
\[
J_1 = \int_{x=0}^{x=1} \arccos x\, x\, dx = \int_{\theta=\pi/2}^{0} \theta\ \cos \theta\ (-\sin \theta d\theta)
= \int_{0}^{\pi/2} \theta \cos \theta \sin \theta\ d\theta
\]

But \(\cos \theta \sin \theta = \frac{1}{2} \sin 2\theta\):

\[
J_1 = \frac{1}{2} \int_{0}^{\pi/2} \theta \sin 2\theta\ d\theta
\]

Let’s use integration by parts:
- Let \(u = \theta\), \(dv = \sin 2\theta d\theta\)
- \(du = d\theta\), \(v = -\frac{1}{2} \cos 2\theta\)

So:
\[
\frac{1}{2} \left[ -\frac{1}{2} \theta \cos 2\theta \Big|_{0}^{\pi/2} + \frac{1}{2} \int_{0}^{\pi/2} \cos 2\theta d\theta \right]
= -\frac{1}{4} \theta \cos 2\theta \Big|_{0}^{\pi/2} + \frac{1}{4} \int_{0}^{\pi/2} \cos 2\theta d\theta
\]

Compute the terms:

1. \(-\frac{1}{4} \theta \cos 2\theta \Big|_{0}^{\pi/2}\):

- At \(\theta = \pi/2\): \(-\frac{1}{4} \frac{\pi}{2} \cos(\pi) = -\frac{1}{4} \frac{\pi}{2} \cdot (-1) = \frac{\pi}{8}\)
- At \(\theta = 0\): \(-\frac{1}{4} \cdot 0 \cdot \cos 0 = 0\)

So the definite part is \(\frac{\pi}{8} - 0 = \frac{\pi}{8}\).

2. \(\frac{1}{4} \int_{0}^{\pi/2} \cos 2\theta d\theta = \frac{1}{4} \left[ \frac{1}{2} \sin 2\theta \Big|_{0}^{\pi/2} \right]\)

At \(\theta = \pi/2\): \(\sin(\pi) = 0\)

At \(\theta = 0\): \(\sin(0) = 0\)

Difference is zero.

Thus,
\[
J_1 = \frac{\pi}{8}
\]

So,
\[
\frac{dI}{d\alpha} = \frac{\pi}{8} - 2\alpha \int_{0}^{1} \arccos x\, x^2\, \mathbf{D}(\alpha x)\ dx
\]

This is an integro-differential equation for \(I(\alpha)\).

At \(\alpha = 0\), \(\mathbf{D}(0) = 0\), so the entire integral is zero:

\[
I(0) = 0
\]

Let’s expand \(I(\alpha)\) in Taylor series for small \(\alpha\):

Suppose
\[
I(\alpha) = A \alpha + B \alpha^3 + \cdots
\]

Plug into the differential equation:

\[
I'(\alpha) = \frac{\pi}{8} - 2\alpha \int_{0}^{1} \arccos x\, x^2\, \mathbf{D}(\alpha x)\ dx
\]

But for small \(\alpha\), \(\mathbf{D}(\alpha x) \approx \alpha x\):

So,
\[
I'(\alpha) \approx \frac{\pi}{8} - 2\alpha \int_{0}^{1} \arccos x\, x^2 \, (\alpha x) dx = \frac{\pi}{8} - 2\alpha^2 \int_{0}^1 \arccos x\, x^3 dx
\]

Integrate \(I'(\alpha)\) to get \(I(\alpha)\):

\[
I(\alpha) \approx \frac{\pi}{8} \alpha - \frac{2}{3} \alpha^3 \int_{0}^1 \arccos x\, x^3 dx
\]

But let's compute this last integral \(J_2 = \int_0^1 \arccos x\, x^3 dx\):

Let \(x = \cos \theta\), \(dx = -\sin\theta d\theta\)

Limits: \(x = 0 \to \theta = \pi/2\), \(x = 1 \to \theta = 0\)

\(x^3 = \cos^3 \theta\)

Thus,
\[
J_2 = \int_{x=0}^{x=1} \arccos x\, x^3 dx = \int_{\theta = \pi/2}^0 \theta \cos^3 \theta (-\sin\theta d\theta) = \int_0^{\pi/2} \theta \cos^3 \theta \sin\theta d\theta
\]

But \(\cos^3 \theta \sin\theta d\theta = \sin\theta (1 - \sin^2 \theta)^{3/2}\) * but that's more complicated than necessary.

Alternatively, use \(\sin\theta \cos^3\theta = \frac{1}{4} \sin 2\theta (1+\cos2\theta)\):

But let's expand, or we can just note that the leading term in the expansion is proportional to \(\alpha\). Since we are not seeing an elementary closed form, let's go back to the direct substitution and see if the integral can be further simplified.

### Step 4: Direct Calculation with Series Expansion for Dawson's Function

Recall:
\[
\mathbf{D}(z) = z - \frac{2}{3} z^3 + \frac{4}{15} z^5 - \ldots
\]
Thus,
\[
\mathbf{D}(0.5x) = 0.5x - \frac{2}{3} \cdot (0.5x)^3 + \frac{4}{15} (0.5x)^5 - \cdots
= 0.5x - \frac{1}{12} x^3 + \frac{1}{120} x^5 - \ldots
\]

Thus,
\[
I = \int_{0}^{1} \arccos x\, \left(0.5x - \frac{1}{12} x^3 + \frac{1}{120} x^5 - \cdots \right) dx
= 0.5 \int_{0}^{1} \arccos x\, x\, dx - \frac{1}{12} \int_{0}^{1} \arccos x\, x^3 dx + \frac{1}{120} \int_{0}^{1} \arccos x\, x^5 dx - \cdots
\]

Let’s denote:
\[
J_n = \int_0^1 \arccos x\, x^n dx
\]
We already computed \(J_1 = \frac{\pi}{8}\) above.

Let's compute \(J_3\):

Let \(x = \cos\theta\), \(dx = -\sin\theta d\theta\), when \(x=0\), \(\theta = \pi/2\), \(x=1\), \(\theta=0\):

\[
J_3 = \int_{x=0}^{x=1} \arccos x\, x^3 dx = \int_{\theta = \pi/2}^{0} \theta \cos^3 \theta (-\sin\theta d\theta) = \int_0^{\pi/2} \theta \cos^3\theta \sin\theta d\theta
\]

Let’s write \(\cos^3 \theta \sin\theta = (\sin \theta) (\cos \theta)^3\).

Let’s use the substitution \(u = \cos \theta\), \(du = -\sin\theta d\theta\):

When \(\theta = 0\): \(u = 1\), \(\theta = \pi/2\): \(u=0\)

So,
\[
J_3 = \int_{\theta=0}^{\pi/2} \theta (\cos\theta)^3 \sin\theta d\theta
\]

But perhaps a recursive formula can be found.

Alternatively, from an integral table (Gradshteyn & Ryzhik 3.621.1), for \(n \geq 0\),
\[
\int_0^1 \arccos x \, x^n dx = \frac{\pi}{2(n+1)}\, {}_2F_1\left(\frac{1}{2}, 1; n+2; 1\right)
\]

Alternatively, let's try to use integration by parts on \(J_n\):

Let \(u = \arccos x\), \(dv = x^n dx\), then \(du = -\frac{1}{\sqrt{1 - x^2}} dx\), \(v = \frac{x^{n+1}}{n+1}\):

\[
J_n = \left. \arccos x \frac{x^{n+1}}{n+1} \right|_0^1 + \frac{1}{n+1} \int_0^1 \frac{x^{n+1}}{\sqrt{1 - x^2}} dx
\]

\(\arccos 1 = 0\), at \(x=1\): term is zero.

At \(x=0\): \(\arccos 0 = \frac{\pi}{2}\), so:

\[
\left. \arccos x \frac{x^{n+1}}{n+1} \right|_0^1 = 0 - \frac{\pi}{2} \cdot 0 = 0
\]

So only the integral term survives:

\[
J_n = \frac{1}{n+1} \int_0^1 \frac{x^{n+1}}{\sqrt{1 - x^2}} dx
\]

But \( \int_0^1 \frac{x^{m}}{\sqrt{1 - x^2}} dx = \frac{1}{2} B\left(\frac{m+1}{2}, \frac{1}{2}\right) = \frac{\Gamma\left(\frac{m+1}{2}\right) \Gamma\left(\frac{1}{2}\right)}{2\Gamma\left(\frac{m+2}{2}\right)} \)

And \( \Gamma(1/2) = \sqrt{\pi} \).

For \( m = n+1 \), this gives:

\[
\int_0^1 \frac{x^{n+1}}{\sqrt{1 - x^2}} dx = \frac{1}{2} B\left(\frac{n+2}{2}, \frac{1}{2}\right)
\]

So,

\[
J_n = \frac{1}{n+1} \cdot \frac{1}{2} \cdot \frac{\Gamma\left(\frac{n+2}{2}\right) \Gamma\left(\frac{1}{2}\right)}{\Gamma\left(\frac{n+3}{2}\right)}
\]

But actually, check the formula for the beta function:

\[
\int_0^1 x^{p-1}(1-x)^{q-1} dx = B(p, q) = \frac{\Gamma(p) \Gamma(q)}{\Gamma(p+q)}
\]

But for our integrals,

\[
I_k = \int_0^1 \frac{x^k}{\sqrt{1 - x^2}} dx
\]

Let’s use the substitution \(x = \sin \phi\), \(dx = \cos \phi d\phi\), \(x^k = \sin^k \phi\), so:

\[
I_k = \int_{x=0}^{x=1} \frac{x^k}{\sqrt{1 - x^2}} dx = \int_{\phi=0}^{\phi=\pi/2} \sin^k \phi\, d\phi
\]

This is a standard integral:

\[
\int_0^{\pi/2} \sin^m \phi\, d\phi = \frac{\sqrt{\pi}\, \Gamma\left( \frac{m+1}{2} \right)}{2 \Gamma\left( \frac{m}{2} + 1\right)}
\]

Therefore,

\[
J_n = \frac{1}{n+1} \int_0^{1} \frac{x^{n+1}}{\sqrt{1 - x^2}} dx = \frac{1}{n+1} \int_0^{\pi/2} \sin^{n+1} \phi\, d\phi = \frac{1}{n+1} \cdot \frac{\sqrt{\pi}\, \Gamma\left( \frac{n+2}{2} \right)}{2 \Gamma\left( \frac{n+3}{2} \right)}
\]

Let’s sum up:

- \(J_n = \frac{\sqrt{\pi}}{2(n+1)} \frac{\Gamma\left(\frac{n+2}{2}\right)}{\Gamma\left(\frac{n+3}{2}\right)}\)

Let’s apply it for \(n = 1, 3, 5\):

- \(J_1 = \frac{\sqrt{\pi}}{4}\frac{\Gamma(1.5)}{\Gamma(2)}\)

But:
- \(\Gamma(1.5) = \frac{1}{2}\sqrt{\pi}\)
- \(\Gamma(2) = 1!\ = 1\)

So,
\[
J_1 = \frac{\sqrt{\pi}}{4} \cdot \frac{1}{2} \sqrt{\pi} = \frac{\pi}{8}
\]
(Agrees with our earlier calculation.)

Now, \(J_3\):

- \(J_3 = \frac{\sqrt{\pi}}{8} \frac{\Gamma(2.5)}{\Gamma(3)}\)
- \(\Gamma(2.5) = \frac{1}{2} \cdot \frac{3}{2} \sqrt{\pi} = \frac{3}{4} \sqrt{\pi}\)
- \(\Gamma(3) = 2!\ = 2\)

So,
\[
J_3 = \frac{\sqrt{\pi}}{8} \cdot \frac{3}{4} \frac{\sqrt{\pi}}{2} = \frac{3 \pi}{64}
\]

Now, \(J_5\):

- \(J_5 = \frac{\sqrt{\pi}}{12} \frac{\Gamma(3.5)}{\Gamma(4)}\)
- \(\Gamma(3.5) = \frac{3}{2} \cdot \frac{1}{2} \cdot \frac{1}{2} \sqrt{\pi} \cdot \Gamma(2)\)
    - In general: \(\Gamma(z+1) = z \Gamma(z)\)
    - \(\Gamma(3.5) = 2.5 \Gamma(2.5) = 2.5 \cdot \frac{3}{4} \sqrt{\pi} = \frac{15}{8} \sqrt{\pi}\)
- \(\Gamma(4) = 3! = 6\)

So,
\[
J_5 = \frac{\sqrt{\pi}}{12} \cdot \frac{15}{8} \frac{\sqrt{\pi}}{6} = \frac{15\pi}{576}
\]

### Now Substitute Back

Recall:
\[
I = 0.5 J_1 - \frac{1}{12} J_3 + \frac{1}{120} J_5 + \cdots
\]
Plug in values:

- \(J_1 = \frac{\pi}{8}\)
- \(J_3 = \frac{3\pi}{64}\)
- \(J_5 = \frac{15\pi}{576}\)

So:

\[
I \approx 0.5 \cdot \frac{\pi}{8} - \frac{1}{12} \cdot \frac{3\pi}{64} + \frac{1}{120} \cdot \frac{15\pi}{576}
\]
Compute each term:

1. \(0.5 \cdot \frac{\pi}{8} = \frac{\pi}{16}\)
2. \(\frac{1}{12} \cdot \frac{3\pi}{64} = \frac{3\pi}{768}\)
3. \(\frac{1}{120} \cdot \frac{15\pi}{576} = \frac{15\pi}{69120} = \frac{\pi}{4608}\)

Sum:

\[
I \approx \frac{\pi}{16} - \frac{3\pi}{768} + \frac{\pi}{4608}
\]

Let’s compute common denominator:

- LCD = 4608
- \(\frac{\pi}{16} = \frac{288\pi}{4608}\)
- \(\frac{3\pi}{768} = \frac{18\pi}{4608}\)
- \(\frac{\pi}{4608}\)

So sum:

\[
I \approx \frac{288\pi - 18\pi + 1\pi}{4608} = \frac{271\pi}{4608}
\]

Now let’s check the value numerically:
- \(\pi \approx 3.14159265358979\)
- \(271\pi \approx 851.97963912\)
- \(851.97963912 / 4608 \approx 0.1848892066\)

But recall this is only up to the \(x^5\) term (three terms). The higher order terms are much smaller, so this is quite accurate.

### Step 5: Summing the Series for More Precision

Let’s add the next term.

- For \(n=7\), \(J_7\):

\[
J_7 = \frac{\sqrt{\pi}}{16} \frac{\Gamma(4.5)}{\Gamma(5)}
\]
But,
- \(\Gamma(5) = 24\)
- \(\Gamma(4.5) = 3.5 \Gamma(3.5) = 3.5 \cdot \frac{15}{8}\sqrt{\pi} = \frac{52.5}{8} \sqrt{\pi} = 6.5625 \sqrt{\pi}\)

Thus,
\[
J_7 = \frac{\sqrt{\pi}}{16} \cdot \frac{6.5625 \sqrt{\pi}}{24} = \frac{6.5625 \pi}{16 \cdot 24} = \frac{6.5625 \pi}{384} = \frac{105 \pi}{6144}
\]

But note: \(0.5^{7} = 1/128\), so the next term is very small:

- Coefficient for \(x^7\) term is:
    - Dawson: next term is \((0.5x)^7 \cdot (\text{some rational})\). In the Taylor expansion, the coefficient for \(x^7\) is \(-8/315\) for \(\mathbf{D}(z)\), so at \(0.5x\), it's:
    \[
    -\frac{8}{315}(0.5x)^7 = -\frac{8}{315} \cdot \frac{1}{128} x^7 = -\frac{1}{5040} x^7
    \]
So, the term is \(-\frac{1}{5040} J_7\):

- \(-\frac{1}{5040} \cdot \frac{105 \pi}{6144} = -\frac{105 \pi}{5040 \cdot 6144} = -\frac{\pi}{294912}\)

Add this to the total:

- From previous sum: \(\frac{271\pi}{4608}\)
- Now subtract \(\frac{\pi}{294912} \approx 0.0000106531\) (using \(\pi \approx 3.14159\)), tiny correction.

So, the first three terms already give 6 decimals of accuracy.

### Step 6: Final Analytical Answer

Hence, the exact answer, up to as many terms as desired, is:
\[
I = \frac{\pi}{16} - \frac{3\pi}{768} + \frac{\pi}{4608} - \frac{\pi}{294912} + \cdots
\]

Or, more generally,
\[
I = \sum_{k=0}^{\infty} c_k J_{2k+1}
\]
where the coefficients \(c_k\) are from the Taylor expansion of the Dawson function \(\mathbf{D}(z)\) at \(z=0\), evaluated at \(z = 0.5x\).

But the sum:
\[
I = \frac{\pi}{16} - \frac{3\pi}{768} + \frac{\pi}{4608} - \frac{\pi}{294912} + \cdots
\]

Or, to compact it, since the coefficients are known, express analytically as:

\[
I = \sum_{k=0}^{\infty} a_k\, J_{2k+1}
\]
with \(a_0 = 0.5\), \(a_1=-1/12\), \(a_2=1/120\), \(a_3=-1/5040\), etc.

### Step 7: Final JSON Output

Here is the answer in JSON format:

```json
{"answer": "\\frac{\\pi}{16} - \\frac{3\\pi}{768} + \\frac{\\pi}{4608} - \\frac{\\pi}{294912}", "numerical_answer": "0.1848785535"}
```