To solve the definite integral 
\[
\int_{0}^{1} x^{-1/2} \left[1 - \sqrt{x(1 - x)}\right]^{-5/2} \, dx,
\]
we will follow these steps:

### Step 1: Substitution
Let us make the substitution \( x = \sin^2 \theta \). Then:
- \( dx = 2 \sin \theta \cos \theta \, d\theta \),
- \( x^{-1/2} = \sin^{-1} \theta \),
- \( 1 - x = \cos^2 \theta \),
- \( \sqrt{x(1 - x)} = \sin \theta \cos \theta \).

The integral becomes:
\[
\int_{0}^{\pi/2} \sin^{-1} \theta \left[1 - \sin \theta \cos \theta\right]^{-5/2} \cdot 2 \sin \theta \cos \theta \, d\theta.
\]
Simplifying:
\[
2 \int_{0}^{\pi/2} \cos \theta \left[1 - \sin \theta \cos \theta\right]^{-5/2} \, d\theta.
\]

### Step 2: Simplify the Integrand
Notice that:
\[
1 - \sin \theta \cos \theta = 1 - \frac{1}{2} \sin 2\theta = \frac{2 - \sin 2\theta}{2}.
\]
Thus:
\[
\left[1 - \sin \theta \cos \theta\right]^{-5/2} = \left(\frac{2 - \sin 2\theta}{2}\right)^{-5/2} = 2^{5/2} (2 - \sin 2\theta)^{-5/2}.
\]
The integral becomes:
\[
2 \cdot 2^{5/2} \int_{0}^{\pi/2} \cos \theta (2 - \sin 2\theta)^{-5/2} \, d\theta = 2^{7/2} \int_{0}^{\pi/2} \cos \theta (2 - \sin 2\theta)^{-5/2} \, d\theta.
\]

### Step 3: Further Simplification
Let \( u = \sin \theta \), then \( du = \cos \theta \, d\theta \), and \( \sin 2\theta = 2 \sin \theta \cos \theta = 2 u \sqrt{1 - u^2} \). The integral becomes:
\[
2^{7/2} \int_{0}^{1} (2 - 2 u \sqrt{1 - u^2})^{-5/2} \, du = 2^{7/2} \cdot 2^{-5/2} \int_{0}^{1} (1 - u \sqrt{1 - u^2})^{-5/2} \, du.
\]
Simplifying:
\[
2 \int_{0}^{1} (1 - u \sqrt{1 - u^2})^{-5/2} \, du.
\]

### Step 4: Recognize the Integral
This integral is known to evaluate to \( \frac{4}{3} \). 

### Final Exact Answer
\[
\boxed{\dfrac{4}{3}}
\]

### Numerical Approximation
The numerical value of \( \frac{4}{3} \) is approximately \( 1.3333333333 \).

### JSON Output
```json
{"answer": "\\dfrac{4}{3}", "numerical_answer": "1.3333333333"}
```