

To solve the definite integral \(\int_{420}^{1672}\frac{\sqrt{\ln(2023-x)}}{\sqrt{\ln(2023-x)}+\sqrt{\ln(x-69)}}\,\mathrm{d}x\), we use symmetry and substitution.

### Step 1: Identify Symmetry
Let \(f(x) = \frac{\sqrt{\ln(2023-x)}}{\sqrt{\ln(2023-x)}+\sqrt{\ln(x-69)}}\). Consider the substitution \(x' = 2092 - x\) (where \(2092 = 420 + 1672\), the sum of the limits of integration). This substitution maps the interval \([420, 1672]\) to itself because:
- When \(x = 420\), \(x' = 2092 - 420 = 1672\),
- When \(x = 1672\), \(x' = 2092 - 1672 = 420\).

### Step 2: Analyze \(f(2092 - x)\)
Compute \(f(2092 - x)\):
\[
f(2092 - x) = \frac{\sqrt{\ln(2023 - (2092 - x))}}{\sqrt{\ln(2023 - (2092 - x))} + \sqrt{\ln((2092 - x) - 69)}}.
\]
Simplify the arguments of the logarithms:
- \(2023 - (2092 - x) = x - 69\),
- \((2092 - x) - 69 = 2023 - x\).

Thus:
\[
f(2092 - x) = \frac{\sqrt{\ln(x - 69)}}{\sqrt{\ln(x - 69)} + \sqrt{\ln(2023 - x)}}.
\]

### Step 3: Sum \(f(x)\) and \(f(2092 - x)\)
Adding \(f(x)\) and \(f(2092 - x)\):
\[
f(x) + f(2092 - x) = \frac{\sqrt{\ln(2023 - x)}}{\sqrt{\ln(2023 - x)} + \sqrt{\ln(x - 69)}} + \frac{\sqrt{\ln(x - 69)}}{\sqrt{\ln(x - 69)} + \sqrt{\ln(2023 - x)}} = 1.
\]

### Step 4: Evaluate the Integral
Let \(I = \int_{420}^{1672} f(x)\,\mathrm{d}x\). Using the substitution \(x' = 2092 - x\), we have:
\[
I = \int_{420}^{1672} f(2092 - x)\,\mathrm{d}x.
\]
Adding the two expressions for \(I\):
\[
2I = \int_{420}^{1672} \left[f(x) + f(2092 - x)\right]\,\mathrm{d}x = \int_{420}^{1672} 1\,\mathrm{d}x = 1672 - 420 = 1252.
\]
Thus, \(I = \frac{1252}{2} = 626\).

### Numerical Approximation
The exact value is \(626\), so the numerical approximation is \(626.0000000000\).

{"answer": "626", "numerical_answer": "626.0000000000"}