

To solve the definite integral \(\int\limits_0^{2} x^{1 - 3/2}(2 - x)^{1 - 1/2}[1 - 0.5x(2 - x)]^{-1} \, dx\), we proceed as follows:

### Step 1: Simplify the integrand
First, simplify the exponents:
- \(1 - \frac{3}{2} = -\frac{1}{2}\), so \(x^{1 - 3/2} = x^{-1/2}\).
- \(1 - \frac{1}{2} = \frac{1}{2}\), so \((2 - x)^{1 - 1/2} = (2 - x)^{1/2}\).

The integrand becomes:
\[
x^{-1/2}(2 - x)^{1/2} \cdot \left[1 - 0.5x(2 - x)\right]^{-1}
\]

### Step 2: Substitution \(t = \frac{x}{2}\)
Let \(x = 2t\), so \(dx = 2dt\). When \(x = 0\), \(t = 0\); when \(x = 2\), \(t = 1\). Substituting:
- \(x^{-1/2} = (2t)^{-1/2} = 2^{-1/2}t^{-1/2}\),
- \((2 - x)^{1/2} = (2 - 2t)^{1/2} = 2^{1/2}(1 - t)^{1/2}\),
- \(1 - 0.5x(2 - x) = 1 - 2t(1 - t) = 1 - 2t + 2t^2\).

The integral transforms to:
\[
\int_0^1 2^{-1/2}t^{-1/2} \cdot 2^{1/2}(1 - t)^{1/2} \cdot \frac{1}{1 - 2t + 2t^2} \cdot 2 \, dt = 2 \int_0^1 t^{-1/2}(1 - t)^{1/2} \cdot \frac{1}{1 - 2t + 2t^2} \, dt
\]

### Step 3: Substitution \(u = 2t - 1\)
Let \(u = 2t - 1\), so \(t = \frac{u + 1}{2}\) and \(dt = \frac{du}{2}\). When \(t = 0\), \(u = -1\); when \(t = 1\), \(u = 1\). Substituting:
- \(t^{-1/2} = \left(\frac{u + 1}{2}\right)^{-1/2} = 2^{1/2}(u + 1)^{-1/2}\),
- \((1 - t)^{1/2} = \left(\frac{1 - u}{2}\right)^{1/2} = 2^{-1/2}(1 - u)^{1/2}\),
- \(1 - 2t + 2t^2 = \frac{(2t - 1)^2 + 1}{2} = \frac{u^2 + 1}{2}\).

The integral becomes:
\[
2 \int_{-1}^1 2^{1/2}(u + 1)^{-1/2} \cdot 2^{-1/2}(1 - u)^{1/2} \cdot \frac{2}{u^2 + 1} \cdot \frac{du}{2} = 2 \int_{-1}^1 \sqrt{\frac{1 - u}{1 + u}} \cdot \frac{1}{u^2 + 1} \, du
\]

### Step 4: Substitution \(v = \sqrt{\frac{1 - u}{1 + u}}\)
Let \(v = \sqrt{\frac{1 - u}{1 + u}}\), so \(u = \frac{1 - v^2}{1 + v^2}\) and \(du = \frac{-4v}{(1 + v^2)^2} dv\). When \(u = -1\), \(v \to \infty\); when \(u = 1\), \(v = 0\). The integrand simplifies to:
\[
\sqrt{\frac{1 - u}{1 + u}} = v, \quad u^2 + 1 = \frac{2(1 + v^4)}{(1 + v^2)^2}
\]

The integral transforms to:
\[
2 \int_0^\infty v \cdot \frac{(1 + v^2)^2}{2(1 + v^4)} \cdot \frac{4v}{(1 + v^2)^2} \, dv = 4 \int_0^\infty \frac{v^2}{1 + v^4} \, dv
\]

### Step 5: Evaluate the standard integral
The integral \(\int_0^\infty \frac{v^2}{1 + v^4} \, dv\) is a standard result. Using the formula for integrals of the form \(\int_0^\infty \frac{x^m}{1 + x^n} \, dx = \frac{\pi}{n} \csc\left(\frac{\pi(m + 1)}{n}\right)\) with \(m = 2\) and \(n = 4\):
\[
\int_0^\infty \frac{v^2}{1 + v^4} \, dv = \frac{\pi}{4} \csc\left(\frac{3\pi}{4}\right) = \frac{\pi}{4} \cdot \sqrt{2} = \frac{\pi}{2\sqrt{2}}
\]

Thus, the original integral is:
\[
4 \cdot \frac{\pi}{2\sqrt{2}} = \sqrt{2}\pi
\]

### Numerical Approximation
The numerical value of \(\sqrt{2}\pi\) is approximately \(4.4428829081\).

{"answer": "\(\sqrt{2}\pi\)", "numerical_answer": "4.4428829081"}