We wish to evaluate

  I = ∫₆₄⁷²⁹ x^(1/2)/(x^(1/2) − x^(1/3)) dx.

Step 1. Express the integrand in a more convenient form.

Notice that
  x^(1/2) = x^(3/6) and x^(1/3) = x^(2/6).

A convenient substitution is
  t = x^(1/6) ⟹ x = t⁶ and dx = 6t⁵ dt.
Also, we then have
  x^(1/2) = t³ and x^(1/3) = t².

The limits change as follows:
  when x = 64, t = 64^(1/6) = 2  (since 2⁶ = 64)
  when x = 729, t = 729^(1/6) = 3  (since 3⁶ = 729).

Thus, in terms of t the integral becomes
  I = ∫₂³ [t³/(t³ − t²)] (6t⁵ dt).

Step 2. Simplify the integrand.

Factor t² from the denominator:
  t³ − t² = t² (t − 1).
Then,
  [t³/(t² (t − 1))] (6t⁵) = 6 t^(3+5-2)/(t − 1) = 6t⁶/(t − 1).

So we now have
  I = 6 ∫₂³ t⁶/(t − 1) dt.

Step 3. Divide the polynomial.

We can write t⁶/(t − 1) by polynomial long division. Observe that

  t⁶/(t − 1) = t⁵ + t⁴ + t³ + t² + t + 1 + 1/(t − 1).

(This follows because (t − 1)(t⁵ + t⁴ + t³ + t² + t + 1) = t⁶ − 1, so t⁶ = (t − 1)(t⁵ + t⁴ + t³ + t² + t + 1) + 1.)

Thus, the integral becomes
  I = 6 ∫₂³ [t⁵ + t⁴ + t³ + t² + t + 1 + 1/(t − 1)] dt.

Break it into two parts:
  I = 6 [∫₂³ (t⁵ + t⁴ + t³ + t² + t + 1) dt + ∫₂³ 1/(t − 1) dt].

Step 4. Compute the antiderivatives.

For the polynomial part:
  ∫ t⁵ dt = t⁶/6, ∫ t⁴ dt = t⁵/5, ∫ t³ dt = t⁴/4,
  ∫ t² dt = t³/3, ∫ t dt = t²/2, ∫ 1 dt = t.
Thus,
  ∫ (t⁵ + t⁴ + t³ + t² + t + 1) dt = t⁶/6 + t⁵/5 + t⁴/4 + t³/3 + t²/2 + t.

For the logarithmic part:
  ∫ 1/(t − 1) dt = ln|t − 1|.

Thus, putting back the factor 6, we have
  I = 6 { [t⁶/6 + t⁵/5 + t⁴/4 + t³/3 + t²/2 + t]₂³ + [ln|t − 1|]₂³ }.

Simplify the 6 multiplied into the first bracket:
  I = [t⁶ + (6/5)t⁵ + (3/2)t⁴ + 2t³ + 3t² + 6t]₂³ + 6[ln|t − 1|]₂³.

Step 5. Evaluate at the limits.

Let F(t) = t⁶ + (6/5)t⁵ + (3/2)t⁴ + 2t³ + 3t² + 6t.

At t = 3:
  3⁶ = 729,
  (6/5)·3⁵ = (6/5)·243 = 1458/5,
  (3/2)·3⁴ = (3/2)·81 = 243/2,
  2·3³ = 2·27 = 54,
  3·3² = 3·9 = 27,
  6·3 = 18.
So, F(3) = 729 + 1458/5 + 243/2 + 54 + 27 + 18.

At t = 2:
  2⁶ = 64,
  (6/5)·2⁵ = (6/5)·32 = 192/5,
  (3/2)·2⁴ = (3/2)·16 = 24,
  2·2³ = 2·8 = 16,
  3·2² = 3·4 = 12,
  6·2 = 12.
So, F(2) = 64 + 192/5 + 24 + 16 + 12 + 12.

Now compute F(3) − F(2):

1. The integer parts:
  (729 + 54 + 27 + 18) − (64 + 24 + 16 + 12 + 12) = (828) − (128) = 700.

2. The fractional parts:
  (1458/5 − 192/5) = 1266/5  and  (243/2) remains.

Thus, F(3) − F(2) = 700 + 1266/5 + 243/2.

For the logarithm part:
  6 [ln|t − 1|]₂³ = 6 [ln|3 − 1| − ln|2 − 1|] = 6 [ln2 − ln1] = 6 ln2,
since ln1 = 0.

Thus, the total integral is
  I = 700 + 1266/5 + 243/2 + 6 ln2.

Step 6. Express the sum as a single fraction.

Write the constant part 700 + 1266/5 + 243/2 with a common denominator.
The common denominator for 1, 5, and 2 is 10:
  700 = 7000/10,
  1266/5 = (1266×2)/10 = 2532/10,
  243/2 = (243×5)/10 = 1215/10.

Thus,
  700 + 1266/5 + 243/2 = (7000 + 2532 + 1215)/10 = 10747/10.

Finally, the integral becomes
  I = (10747/10) + 6 ln2.

Step 7. Provide a numerical approximation.

First, note that
  10747/10 = 1074.7,
and ln2 ≈ 0.6931471805599453 so that
  6 ln2 ≈ 6 × 0.6931471805599453 ≈ 4.158883083359672.

Thus,
  I ≈ 1074.7 + 4.158883083359672 = 1078.8588830833597.

Rounded to 10 decimal places, the numerical answer is
  1078.8588830834.

Final Answer in the required JSON format:
{"answer": "\\frac{10747}{10}+6\\ln(2)", "numerical_answer": "1078.8588830834"}