To evaluate the definite integral

$$
\int_0^1 x^{-3/4}(1 - x)^{-1/4}\left[1 - \sqrt{x(1 - x)}\right]^{-2} dx,
$$

we begin by observing the structure of the integrand. It contains powers of $ x $ and $ 1 - x $, as well as a term involving the square root of their product raised to a negative power. This suggests that the integral may be expressible in terms of special functions like the Beta or Gamma function.

---

### Step 1: Series Expansion of the Denominator

We note that the term $ [1 - \sqrt{x(1 - x)}]^{-2} $ can be expanded using the binomial series for $ (1 - y)^{-2} $, valid for $ |y| < 1 $:

$$
(1 - y)^{-2} = \sum_{k=0}^\infty (k + 1) y^k.
$$

Here, $ y = \sqrt{x(1 - x)} $, and since $ x(1 - x) \leq \frac{1}{4} $, we have $ \sqrt{x(1 - x)} \leq \frac{1}{2} < 1 $, so the series converges for all $ x \in [0,1] $.

Substituting into the integral:

$$
\int_0^1 x^{-3/4}(1 - x)^{-1/4} \sum_{k=0}^\infty (k + 1) [x(1 - x)]^{k/2} dx.
$$

Interchange of summation and integration is justified by uniform convergence, leading to:

$$
\sum_{k=0}^\infty (k + 1) \int_0^1 x^{-3/4 + k/2}(1 - x)^{-1/4 + k/2} dx.
$$

This is now a standard Beta function integral:

$$
\int_0^1 x^{a - 1}(1 - x)^{b - 1} dx = B(a, b) = \frac{\Gamma(a)\Gamma(b)}{\Gamma(a + b)},
$$

where $ a = \frac{k}{2} + \frac{1}{4} $, $ b = \frac{k}{2} + \frac{3}{4} $, and $ a + b = k + 1 $.

Thus, the integral becomes:

$$
\sum_{k=0}^\infty (k + 1) \cdot \frac{\Gamma\left(\frac{k}{2} + \frac{1}{4}\right) \Gamma\left(\frac{k}{2} + \frac{3}{4}\right)}{\Gamma(k + 1)}.
$$

---

### Step 2: Use of Gamma Function Identities

Using the **Legendre duplication formula**:

$$
\Gamma(z)\Gamma\left(z + \frac{1}{2}\right) = 2^{1 - 2z} \sqrt{\pi} \Gamma(2z),
$$

we apply it with $ z = \frac{k}{2} + \frac{1}{4} $, which gives:

$$
\Gamma\left(\frac{k}{2} + \frac{1}{4}\right) \Gamma\left(\frac{k}{2} + \frac{3}{4}\right) = 2^{1 - 2\left(\frac{k}{2} + \frac{1}{4}\right)} \sqrt{\pi} \Gamma(k + \frac{1}{2}).
$$

Simplifying the exponent:

$$
1 - 2\left(\frac{k}{2} + \frac{1}{4}\right) = 1 - k - \frac{1}{2} = \frac{1}{2} - k.
$$

So the product becomes:

$$
2^{\frac{1}{2} - k} \sqrt{\pi} \Gamma(k + \frac{1}{2}).
$$

Thus, the sum becomes:

$$
\sum_{k=0}^\infty (k + 1) \cdot \frac{2^{\frac{1}{2} - k} \sqrt{\pi} \Gamma(k + \frac{1}{2})}{\Gamma(k + 1)}.
$$

Recall that $ \Gamma(k + 1) = k! $, and $ \Gamma(k + \frac{1}{2}) $ has a known expression:

$$
\Gamma(k + \frac{1}{2