We start with

  I = ∫₀¹ (x - 1)² (x + 1)² (x² + 1)² (x⁴ + 1)² dx.

Notice that
  (x - 1)² (x + 1)² = (x² - 1)².

Then we have
  I = ∫₀¹ (x² - 1)² (x² + 1)² (x⁴ + 1)² dx.

Next, note that
  (x² - 1)(x² + 1) = x⁴ - 1,
so that
  (x² - 1)² (x² + 1)² = (x⁴ - 1)².

Thus, the integrand becomes
  (x⁴ - 1)² (x⁴ + 1)² = [(x⁴ - 1)(x⁴ + 1)]² = (x⁸ - 1)².

Since (x⁸ - 1)² = (1 - x⁸)², we can write
  I = ∫₀¹ (1 - x⁸)² dx.

Expanding (1 - x⁸)² gives:
  (1 - x⁸)² = 1 - 2x⁸ + x¹⁶.

We integrate term by term:
  ∫₀¹ 1 dx = 1,
  ∫₀¹ 2x⁸ dx = 2·(1/9) = 2/9,
  ∫₀¹ x¹⁶ dx = 1/17.

So,
  I = 1 - (2/9) + (1/17).

To combine these fractions, write them with a common denominator (the least common multiple of 9 and 17 is 153):
  1 = 153/153,
  2/9 = 34/153,
  1/17 = 9/153.

Thus:
  I = (153 - 34 + 9) / 153 = 128 / 153.

For a numerical approximation:
  128 ÷ 153 ≈ 0.8366013072.

Thus, the final answer is:
{"answer": "\\frac{128}{153}", "numerical_answer": "0.8366013072"}