We wish to evaluate

  I = ∫₁² (2^(x–1) + log₂(2x)) dx.

Step 1. Write the integral as the sum of two integrals:
  I = I₁ + I₂
where
  I₁ = ∫₁² 2^(x–1) dx  and  I₂ = ∫₁² log₂(2x) dx.

Step 2. Evaluate I₁:
Notice that
  2^(x–1) = 2^x / 2.
Thus,
  I₁ = (1/2) ∫₁² 2^x dx.
Recall that ∫ 2^x dx = 2^x / ln2, so
  I₁ = (1/2) [2^x/ln2] (evaluated from 1 to 2)
    = (1/(2 ln2)) (2² – 2¹)
    = (1/(2 ln2)) (4 – 2)  = (1/(2 ln2)) (2)
    = 1/ln2.

Step 3. Evaluate I₂:
Write log₂(2x) in terms of the natural logarithm:
  log₂(2x) = ln(2x)/ln2.
Then,
  I₂ = (1/ln2) ∫₁² ln(2x) dx.
Make the substitution:
  Let u = 2x ⇒ du = 2 dx ⇒ dx = du/2.
When x = 1, u = 2; when x = 2, u = 4.
Thus, the integral becomes:
  I₂ = (1/ln2)(1/2) ∫₂⁴ ln u du.
Recall that ∫ ln u du = u ln u – u.
Then,
  ∫₂⁴ ln u du = [u ln u – u] from 2 to 4:
    = (4 ln4 – 4) – (2 ln2 – 2)
    = 4 ln4 – 4 – 2 ln2 + 2
    = 4 ln4 – 2 ln2 – 2.
Since ln4 = 2 ln2, we have:
  4 ln4 = 4 (2 ln2) = 8 ln2.
Thus,
  I₂ = (1/(2 ln2)) (8 ln2 – 2 ln2 – 2)
    = (1/(2 ln2)) (6 ln2 – 2)
    = (6 ln2 – 2)/(2 ln2)
    = (2(3 ln2 –1))/(2 ln2)
    = (3 ln2 –1)/ln2.

Step 4. Combine I₁ and I₂:
  I = I₁ + I₂ = (1/ln2) + ((3 ln2 –1)/ln2)
    = (1 + 3 ln2 – 1)/ln2   [since 1 – 1 cancels]
    = (3 ln2)/ln2
    = 3.

Step 5. Numerical approximation: Since 3 is exact, the numerical value is 3.0000000000.

Thus, the final answer is as follows:
{"answer": "$3$", "numerical_answer": "3.0000000000"}