Let's solve the integral:
\[
I = \int_0^1 \sqrt[4]{\frac{1}{x} - 1} \, dx.
\]

**Step 1: Simplify the Integrand**

Letâ€™s write \(\frac{1}{x} - 1 = \frac{1-x}{x}\), so
\[
I = \int_0^1 \left( \frac{1-x}{x} \right)^{1/4} dx = \int_0^1 \frac{(1-x)^{1/4}}{x^{1/4}} dx.
\]

\[
I = \int_0^1 (1-x)^{1/4} x^{-1/4} dx.
\]

**Step 2: Recognize as Beta Integral**

The Beta function is defined as:
\[
B(a, b) = \int_0^1 x^{a-1} (1-x)^{b-1} dx = \frac{\Gamma(a) \Gamma(b)}{\Gamma(a+b)}
\]

Here, 
- \(a - 1 = -\frac{1}{4} \implies a = \frac{3}{4}\)
- \(b - 1 = \frac{1}{4} \implies b = \frac{5}{4}\)

So our integral is:
\[
I = \int_0^1 (1-x)^{1/4} x^{-1/4} dx = B\left(\frac{3}{4}, \frac{5}{4}\right)
\]

**Step 3: Use Gamma Functions**

So,
\[
I = \frac{\Gamma\left(\frac{3}{4}\right)\Gamma\left(\frac{5}{4}\right)}{\Gamma\left(2\right)}
\]
But \(\Gamma(2) = 1!\) = 1, so:
\[
I = \Gamma\left(\frac{3}{4}\right) \Gamma\left(\frac{5}{4}\right)
\]

Now, relate \(\Gamma\left(\frac{5}{4}\right)\) to \(\Gamma\left(\frac{1}{4}\right)\) using \(\Gamma(z+1) = z\Gamma(z)\):
\[
\Gamma\left(\frac{5}{4}\right) = \frac{1}{4} \Gamma\left(\frac{1}{4}\right)
\]

So,
\[
I = \Gamma\left(\frac{3}{4}\right) \cdot \frac{1}{4} \Gamma\left(\frac{1}{4}\right) = \frac{1}{4} \Gamma\left(\frac{1}{4}\right) \Gamma\left(\frac{3}{4}\right)
\]

**Step 4: Final Exact Answer**

\[
\boxed{
I = \frac{1}{4} \Gamma\left(\frac{1}{4}\right) \Gamma\left(\frac{3}{4}\right)
}
\]

**Step 5: Numerical Value**

We can use the reflection/duplication formulas or look up values:
- \(\Gamma\left(\frac{1}{4}\right) \approx 3.6256099082\)
- \(\Gamma\left(\frac{3}{4}\right) \approx 1.2254167025\)

Thus,
\[
I \approx \frac{1}{4} \times 3.6256099082 \times 1.2254167025 \approx \frac{1}{4} \times 4.4428829382 \approx 1.1107207346
\]

**JSON output:**

```json
{"answer": "\\frac{1}{4} \\Gamma\\left(\\frac{1}{4}\\right)\\Gamma\\left(\\frac{3}{4}\\right)", "numerical_answer": "1.1107207346"}
```