

To calculate the definite integral \(\int_0^6 \left( x + (x-3)^7 + \sin(x-3) \right) dx\), we proceed as follows:

### Step 1: Split the integral into three separate integrals
By linearity of integration, we can split the integral into the sum of three simpler integrals:
\[
\int_0^6 \left( x + (x-3)^7 + \sin(x-3) \right) dx = \int_0^6 x \, dx + \int_0^6 (x-3)^7 \, dx + \int_0^6 \sin(x-3) \, dx
\]

### Step 2: Evaluate \(\int_0^6 x \, dx\)
The antiderivative of \(x\) is \(\frac{1}{2}x^2\). Evaluating from \(0\) to \(6\):
\[
\int_0^6 x \, dx = \left. \frac{1}{2}x^2 \right|_0^6 = \frac{1}{2}(6^2) - \frac{1}{2}(0^2) = \frac{1}{2}(36) - 0 = 18
\]

### Step 3: Evaluate \(\int_0^6 (x-3)^7 \, dx\)
Use the substitution \(u = x - 3\), so \(du = dx\). When \(x = 0\), \(u = -3\); when \(x = 6\), \(u = 3\). The integral becomes:
\[
\int_{-3}^3 u^7 \, du
\]
The antiderivative of \(u^7\) is \(\frac{1}{8}u^8\). Evaluating from \(-3\) to \(3\):
\[
\left. \frac{1}{8}u^8 \right|_{-3}^3 = \frac{1}{8}(3^8) - \frac{1}{8}((-3)^8)
\]
Since \(3^8 = (-3)^8 = 6561\), this simplifies to:
\[
\frac{1}{8}(6561) - \frac{1}{8}(6561) = 0
\]

### Step 4: Evaluate \(\int_0^6 \sin(x-3) \, dx\)
Again, use the substitution \(u = x - 3\), so \(du = dx\). The integral becomes:
\[
\int_{-3}^3 \sin(u) \, du
\]
The antiderivative of \(\sin(u)\) is \(-\cos(u)\). Evaluating from \(-3\) to \(3\):
\[
\left. -\cos(u) \right|_{-3}^3 = -\cos(3) - (-\cos(-3))
\]
Since \(\cos(-3) = \cos(3)\) (cosine is even), this simplifies to:
\[
-\cos(3) + \cos(3) = 0
\]

### Step 5: Combine the results
Adding the three integrals together:
\[
18 + 0 + 0 = 18
\]

### Numerical Approximation
The exact result is \(18\), so the numerical approximation to 10 decimal places is \(18.0000000000\).

{"answer": "18", "numerical_answer": "18.0000000000"}