<think>
Okay, let's tackle this integral step by step. The problem is to compute the definite integral from 0 to infinity of (x²/(e^x - 1)) multiplied by [8 sinh(0.5x) - sinh(0.25x)] dx. Hmm, that looks a bit intimidating at first, but maybe I can break it down.

First, I remember that sinh(a x) can be expressed in terms of exponentials: sinh(ax) = (e^{ax) - e^{-ax}) / 2. So maybe expanding that part will help. Let me write out the entire integrand with that substitution.

So, the integrand becomes x²/(e^x - 1) times [8*(e^{0.5x} - e^{-0.5x})/2 - (e^{0.25x} - e^{-0.25x})/2]. Let me simplify the coefficients here. The 8 multiplied by 1/2 gives 4, and the other term is -1/2. So that simplifies to 4(e^{0.5x} - e^{-0.5x}) - (1/2)(e^{0.25x} - e^{-0.25x}).

Therefore, the integral can be split into two separate integrals: 4 times the integral of x²/(e^x -1)(e^{0.5x} - e^{-0.5x}) dx minus (1/2) times the integral of x²/(e^x -1)(e^{0.25x} - e^{-0.25x}) dx, all from 0 to infinity.

Wait, but maybe I can combine the exponentials in the numerator. Let's see. For the first term, e^{0.5x} - e^{-0.5x} multiplied by 1/(e^x -1). Let me factor that. The denominator is e^x -1, which is e^{x} -1. Let's see if the numerator can be expressed in terms that cancel with the denominator.

Alternatively, perhaps I can write the entire expression as a sum of terms with different exponents. Let me try that. For the first part: 4*(e^{0.5x} - e^{-0.5x}) / (e^x -1). Let's factor e^{-0.5x} in the denominator? Wait, maybe not. Let's see:

The denominator e^x -1 can be written as e^{x} -1. Let's see, e^{0.5x} - e^{-0.5x} is equal to 2( sinh(0.5x) ), but maybe that's not helpful here. Alternatively, let's consider combining the exponentials. Let's take the first term:

4 * [e^{0.5x} - e^{-0.5x}] / (e^x -1) = 4 * [e^{0.5x} - e^{-0.5x}] / (e^{x} -1)

Let me factor e^{-0.5x} from the numerator:

4 * e^{-0.5x} [e^{x} -1] / (e^x -1) ) = 4 e^{-0.5x}

Wait, that's a key insight! Because e^{0.5x} - e^{-0.5x} = e^{-0.5x}(e^{x} -1). So when we divide by (e^x -1), those terms cancel out. Let me check that:

e^{0.5x} - e^{-0.5x} = e^{-0.5x} (e^{x} -1). Let's verify:

e^{-0.5x} * (e^x -1) = e^{0.5x} - e^{-0.5x}. Yes, that's correct. So, that term simplifies to 4 e^{-0.5x}.

Similarly, for the second part: [e^{0.25x} - e^{-0.25x}]/(e^x -1). Let's see if that can be simplified similarly. Let's factor e^{-0.25x} from the numerator:

e^{-0.25x} (e^{0.5x} -1). Wait, e^{0.25x} - e^{-0.25x} = e^{-0.25x}(e^{0.5x} -1). Hmm, but the denominator is e^x -1, which is e^{x} -1. So that's not directly canceling. Wait, perhaps not as straightforward as the first term. Let me check:

Wait, e^{0.25x} - e^{-0.25x} = e^{-0.25x}(e^{0.5x} -1). So when we divide by e^x -1, which is (e^{0.5x})^2 -1 = (e^{0.5x} -1)(e^{0.5x} +1). So, the denominator can be written as (e^{0.5x} -1)(e^{0.5x} +1). Therefore, the term [e^{0.25x} - e^{-0.25x}]/(e^x -1) becomes e^{-0.25x}(e^{0.5x} -1)/[(e^{0.5x} -1)(e^{0.5x} +1)] ) = e^{-0.25x}/(e^{0.5x} +1) = e^{-0.25x}/(e^{0.5x} +1) = e^{-0.25x}/(e^{0.5x} +1). Hmm, that's a better simplification.

So putting this all together, the original integrand becomes:

x²/(e^x -1) [8 sinh(0.5x) - sinh(0.25x)] dx = x² [4 e^{-0.5x} - (1/2) e^{-0.25x}/(e^{0.5x} +1) ] dx.

Wait, but let me confirm. The first term after substitution was 4 e^{-0.5x}, and the second term was -(1/2) times [e^{-0.25x}/(e^{0.5x} +1)].

So the integral becomes:

Integral from 0 to infinity of x² [4 e^{-0.5x} - (1/2) e^{-0.25x}/(e^{0.5x} +1) ] dx.

Hmm, so now we have two separate terms. The first term is 4 x² e^{-0.5x}, which is straightforward to integrate. The second term is - (1/2) x² e^{-0.25x}/(e^{0.5x} +1). Let's handle them one by one.

First integral: 4 ∫₀^∞ x² e^{-0.5x} dx. The integral of x² e^{-a x} dx from 0 to ∞ is 2!/a³. So here, a = 0.5, so the integral is 2!/(0.5)^3 = 2/(1/8) = 16. Then multiplied by 4 gives 4*16 = 64. So that's the first part.

Now the second integral: - (1/2) ∫₀^∞ x² e^{-0.25x}/(e^{0.5x} +1) dx. Let's see. Let me make a substitution here. Let me note that e^{0.5x} = e^{(0.5)x}, and e^{-0.25x} = e^{-0.25x}. So combining exponents: e^{-0.25x}/(e^{0.5x} +1) = e^{-0.25x}/(e^{0.5x} +1 + e^{-0.5x} - e^{-0.5x})? Hmm, maybe not. Alternatively, let's write the denominator as e^{0.5x} +1 = e^{0.5x}(1 + e^{-0.5x}), so then:

e^{-0.25x}/(e^{0.5x} +1) = e^{-0.25x}/(e^{0.5x}(1 + e^{-0.5x})) = e^{-0.25x -0.5x}/(1 + e^{-0.5x}) = e^{-0.75x}/(1 + e^{-0.5x}).

So the second integral becomes - (1/2) ∫₀^∞ x² e^{-0.75x}/(1 + e^{-0.5x}) dx. Let me make a substitution here. Let t = 0.5x, so x = 2t, dx = 2 dt. Then when x=0, t=0; x=∞, t=∞. Substitute:

- (1/2) ∫₀^∞ (2t)^2 e^{-0.75*(2t)}/(1 + e^{-0.5*(2t)}) * 2 dt.

Simplify:

- (1/2) * 4 t² * e^{-1.5t}/(1 + e^{-t}) * 2 dt = - (1/2) *4*2 * ∫₀^∞ t² e^{-1.5t}/(1 + e^{-t}) dt = -4 ∫₀^∞ t² e^{-1.5t}/(1 + e^{-t}) dt.

Hmm, perhaps this is a known integral. Alternatively, note that 1/(1 + e^{-t}) can be expressed as a geometric series. Since e^{-t} <1 for t>0, so 1/(1 + e^{-t}) = Σ_{n=0}^∞ (-1)^n} e^{-n t} }, but wait, actually, the expansion of 1/(1 + e^{-t}) is 1/(1 + e^{-t}) = Σ_{n=0}^∞ (-1)^n e^{-n t} } for |e^{-t}| <1, which is true for t>0. But this is an alternating series. Alternatively, maybe we can write it as Σ_{n=0}^∞ (-1)^n e^{-n t} }.

But let me check: 1/(1 + e^{-t}) = 1 - e^{-t}/(1 + e^{-t})? Hmm, maybe not. Alternatively, 1/(1 + e^{-t}) = Σ_{n=0}^∞ (-1)^n e^{-n t} }, which is the expansion for 1/(1 + e^{-t}) = Σ_{n=0}^∞ (-1)^n e^{-n t} }, valid for e^{-t} <1, which is true for t>0. So that's a valid expansion.

Therefore, the integral becomes:

-4 ∫₀^∞ t² e^{-1.5t} Σ_{n=0}^∞ (-1)^n e^{-n t} dt = -4 Σ_{n=0}^∞ (-1)^n ∫₀^∞ t² e^{-(1.5 + n) t} dt.

Wait, but integrating term by term. The integral of t² e^{-a t} dt from 0 to ∞ is 2! / a³ = 2/a³. So each term in the series would be (-1)^n * 2 / (1.5 + n)^3. Therefore, the second integral becomes:

-4 * 2 Σ_{n=0}^∞ (-1)^n / (n + 1.5)^3 = -8 Σ_{n=0}^∞ (-1)^n / (n + 1.5)^3.

Hmm, this series might be related to the Dirichlet eta function or the Riemann zeta function. The Dirichlet eta function is η(s) = Σ_{n=1}^∞ (-1)^{n+1}/n^s = (1 - 2^{1 - s}) ζ(s). But here, the sum is Σ_{n=0}^∞ (-1)^n / (n + 1.5)^3. Let's shift the index: let m = n +1, so when n=0, m=1. Then Σ_{n=0}^∞ (-1)^n/(n + 1.5)^3 = Σ_{m=1}^∞ (-1)^{m-1}/(m + 0.5)^3 = - Σ_{m=1}^∞ (-1)^m/(m + 0.5)^3. Hmm, not sure if that helps. Alternatively, perhaps express it in terms of the Hurwitz zeta function or the Lerch transcendent.

Alternatively, maybe we can relate it to the Riemann zeta function. Let me recall that Σ_{n=0}^∞ (-1)^n/(n + a)^s = 2^{-s} Φ(-1, s, a), where Φ is the Lerch zeta function. But I'm not sure if that's helpful here. Alternatively, perhaps using integral representations.

Alternatively, maybe we can write this sum as an integral. Let me think. The sum Σ_{n=0}^∞ (-1)^n/(n + a)^s can be expressed using the integral representation of the Hurwitz zeta function. But I might need to look that up. Alternatively, perhaps there's a known value for this sum when s=3 and a=1.5.

Alternatively, maybe we can compute this sum numerically. But since the problem asks for an analytical solution, perhaps there's a way to express this sum in terms of known constants.

Alternatively, let's note that 1.5 is 3/2, so the sum is Σ_{n=0}^∞ (-1)^n/(n + 3/2)^3. Let me see if this can be expressed in terms of the Riemann zeta function or other known functions. Alternatively, perhaps using the integral representation of 1/(n + a)^3.

Recall that 1/(n + a)^3 = (1/2) ∫₀^∞ t² e^{-(n + a) t} dt. So substituting this into the sum:

Σ_{n=0}^∞ (-1)^n/(n + 3/2)^3 = (1/2) Σ_{n=0}^∞ (-1)^n ∫₀^∞ t² e^{-(n + 3/2) t} dt = (1/2) ∫₀^∞ t² e^{-3/2 t} Σ_{n=0}^∞ (-1)^n e^{-n t} dt.

But the sum Σ_{n=0}^∞ (-1)^n e^{-n t} is a geometric series with ratio -e^{-t}, so it sums to 1/(1 + e^{-t}).

Therefore, the sum becomes (1/2) ∫₀^∞ t² e^{-3/2 t} / (1 + e^{-t}) dt. But this is the same integral we started with for the second term, except for constants. Wait, but this seems to be going in circles. Wait, but perhaps this integral can be related to the original integral. Wait, but in our case, the second term was -8 times this sum, which is -8 * [ (1/2) ∫₀^∞ t² e^{-3/2 t}/(1 + e^{-t}) dt ] = -4 ∫₀^∞ t² e^{-3/2 t}/(1 + e^{-t}) dt. But this is the same as the original second integral. So perhaps this approach isn't helpful.

Alternatively, maybe we can split the denominator 1 + e^{-t} into something else. Let me consider substituting u = e^{-t}, then t = -ln u, dt = -du/u. When t=0, u=1; t=∞, u=0. So the integral becomes ∫₀^1 [ (-ln u)^2 ] e^{-3/2 (-ln u)} / (1 + u) * (-du/u). Let's simplify:

e^{-3/2 (-ln u)} = e^{(3/2) ln u} = u^{3/2}. So the integral becomes ∫₁^0 [ (ln u)^2 ] u^{3/2}/(1 + u) * (du/u) ) * (-1) = ∫₀^1 (ln u)^2 u^{1/2}/(1 + u) du.

Hmm, not sure if that helps. Alternatively, perhaps expanding 1/(1 + u) as a power series. Since 1/(1 + u) = Σ_{k=0}^∞ (-1)^k u^k for |u| <1. But u is between 0 and1, so that's valid. Therefore, the integral becomes Σ_{k=0}^∞ (-1)^k ∫₀^1 (ln u)^2 u^{k + 1/2} du.

But integrating (ln u)^2 u^{a} du from 0 to1. Let me recall that ∫₀^1 u^a (ln u)^n du = (-1)^n n! / (a +1)^{n+1} }, for a > -1. So here, a = k +1/2, n=2. Therefore, the integral is (-1)^2 2! / (k + 1/2 +1)^3 = 2 / (k + 3/2)^3.

Therefore, the sum becomes Σ_{k=0}^∞ (-1)^k * 2 / (k + 3/2)^3. But this is exactly the same sum as before, which is 2 Σ_{k=0}^∞ (-1)^k / (k + 3/2)^3. So this approach also leads back to the same sum, which suggests that we can't express it in terms of elementary functions. Hmm, this is a problem.

Alternatively, perhaps there's a different approach to the original integral. Let me go back and see if there's another way to handle the integrand.

Original integral: ∫₀^∞ [x²/(e^x -1)] [8 sinh(0.5x) - sinh(0.25x)] dx.

Wait, another thought: perhaps express the entire integrand in terms of exponentials and then split into terms of the form x² e^{-a x}/(1 - e^{-x}), which can be related to the Riemann zeta function.

Wait, the standard integral ∫₀^∞ x^{s-1}/(e^x -1) dx = Γ(s) ζ(s). But here, we have additional sinh terms. Let me try expanding the sinh terms as exponentials again.

So, 8 sinh(0.5x) - sinh(0.25x) = 8*(e^{0.5x} - e^{-0.5x})/2 - (e^{0.25x} - e^{-0.25x})/2 = 4(e^{0.5x} - e^{-0.5x}) - 0.5(e^{0.25x} - e^{-0.25x}).

Therefore, the integrand becomes x²/(e^x -1) [4(e^{0.5x} - e^{-0.5x}) - 0.5(e^{0.25x} - e^{-0.25x})].

Expanding this, we get four terms:

4x² e^{0.5x}/(e^x -1) -4x² e^{-0.5x}/(e^x -1) -0.5x² e^{0.25x}/(e^x -1) +0.5x² e^{-0.25x}/(e^x -1).

Now, let's consider each term separately. For example, the first term: 4x² e^{0.5x}/(e^x -1) = 4x² e^{0.5x}/(e^x -1) = 4x² e^{-0.5x}/(1 - e^{-x}).

Similarly, e^{0.5x}/(e^x -1) = e^{-0.5x}/(1 - e^{-x}).

Similarly, the second term: -4x² e^{-0.5x}/(e^x -1) = -4x² e^{-0.5x}/(1 - e^{-x}).

Third term: -0.5x² e^{0.25x}/(e^x -1) = -0.5x² e^{-0.75x}/(1 - e^{-x}).

Fourth term: 0.5x² e^{-0.25x}/(e^x -1) = 0.5x² e^{-0.25x}/(1 - e^{-x}).

So now, each term is of the form x² e^{-k x}/(1 - e^{-x}), which can be expressed as x² e^{-k x} Σ_{n=0}^∞ e^{-n x} }, since 1/(1 - e^{-x}) = Σ_{n=0}^∞ e^{-n x} for x>0.

Therefore, each term can be written as a sum of integrals. Let's handle each term:

First term: 4x² e^{-0.5x} Σ_{n=0}^∞ e^{-n x} dx = 4 Σ_{n=0}^∞ ∫₀^∞ x² e^{-(n +0.5)x} dx.

Similarly, the integral of x² e^{-a x} dx from 0 to ∞ is 2/a³. So this term becomes 4 Σ_{n=0}^∞ 2/(n +0.5)^3 = 8 Σ_{n=0}^∞ 1/(n +0.5)^3.

Second term: -4x² e^{-0.5x} Σ_{n=0}^∞ e^{-n x} dx = -4 Σ_{n=0}^∞ ∫₀^∞ x² e^{-(n +0.5)x} dx = -4 Σ_{n=0}^∞ 2/(n +0.5)^3 = -8 Σ_{n=0}^∞ 1/(n +0.5)^3.

Third term: -0.5x² e^{-0.75x} Σ_{n=0}^∞ e^{-n x} dx = -0.5 Σ_{n=0}^∞ ∫₀^∞ x² e^{-(n +0.75)x} dx = -0.5 Σ_{n=0}^∞ 2/(n +0.75)^3 = -1 Σ_{n=0}^∞ 1/(n +0.75)^3.

Fourth term: 0.5x² e^{-0.25x} Σ_{n=0}^∞ e^{-n x} dx = 0.5 Σ_{n=0}^∞ ∫₀^∞ x² e^{-(n +0.25)x} dx = 0.5 Σ_{n=0}^∞ 2/(n +0.25)^3 = 1 Σ_{n=0}^∞ 1/(n +0.25)^3.

So combining all four terms:

First term + Second term + Third term + Fourth term =

8 Σ_{n=0}^∞ 1/(n +0.5)^3 -8 Σ_{n=0}^∞ 1/(n +0.5)^3 - Σ_{n=0}^∞ 1/(n +0.75)^3 + Σ_{n=0}^∞ 1/(n +0.25)^3.

Wait, the first two terms cancel each other out: 8Σ -8Σ =0. So we're left with:

- Σ_{n=0}^∞ 1/(n +0.75)^3 + Σ_{n=0}^∞ 1/(n +0.25)^3.

So the entire integral simplifies to:

Σ_{n=0}^∞ [1/(n +0.25)^3 -1/(n +0.75)^3 ].

Hmm, this is a telescoping series? Not exactly, but perhaps we can relate it to the Hurwitz zeta function, which is defined as ζ(s, a) = Σ_{n=0}^∞ 1/(n +a)^s. So here, s=3, and a=0.25 and a=0.75. Therefore, the integral is ζ(3, 0.25) - ζ(3, 0.75).

But the Hurwitz zeta function can sometimes be expressed in terms of the Riemann zeta function or other special functions. Alternatively, there might be a reflection formula or relation between ζ(3, 0.25) and ζ(3, 0.75). Let me recall that ζ(s, a) + ζ(s, 1 -a) = 2^{s} ζ(s, 2a) when 2a <1? Not sure. Alternatively, perhaps using the identity ζ(s, a) = 2^{s} ζ(s, 2a) + 2^{s} ζ(s, 2a -1). Hmm, not sure. Alternatively, using the relation between the Hurwitz zeta and the polylogarithm function.

Alternatively, perhaps using the integral representation of the Hurwitz zeta function. But I'm not sure. Alternatively, recall that ζ(s, a) can be expressed in terms of the Riemann zeta function for rational a. For example, when a is a fraction like 1/4 or 3/4, there might be known expressions.

Alternatively, using the relation between the Riemann zeta function and the Hurwitz zeta function. For example, ζ(s, a) = Σ_{n=0}^∞ 1/(n +a)^s. So ζ(s, 1/4) - ζ(s, 3/4) = Σ_{n=0}^∞ [1/(n +1/4)^s -1/(n +3/4)^s ].

This can be written as Σ_{k=0}^∞ [1/(k +1/4)^s -1/(k +3/4)^s ] for k from 0 to ∞. Let me change variables: let m = 2k. Hmm, not sure. Alternatively, note that 1/4 and 3/4 sum to 1. So perhaps there's a reflection formula. For example, ζ(s, a) - ζ(s, 1 -a) = ... ?

Alternatively, using the functional equation for the Hurwitz zeta function, but I'm not familiar with such an equation off the top of my head.

Alternatively, perhaps express these sums in terms of the Riemann zeta function multiplied by some factors. For example, ζ(s, 1/4) = 4^s Σ_{n=1}^∞ 1/(4n -3)^s } + 4^s Σ_{n=1}^∞ 1/(4n -0)^s }? Not sure. Alternatively, split the sum into terms modulo 4.

Alternatively, note that ζ(s, 1/4) = Σ_{n=0}^∞ 1/(n +1/4)^s = Σ_{m=1/4, 5/4, 9/4,...} 1/m^s. Similarly, ζ(s, 3/4) = Σ_{m=3/4, 7/4, 11/4,...} 1/m^s. So the difference ζ(s,1/4) - ζ(s,3/4) = Σ_{k=0}^∞ [1/(k +1/4)^s -1/(k +3/4)^s ].

This can be written as Σ_{k=0}^∞ [1/( (4k +1)/4 )^s -1/( (4k +3)/4 )^s ] = 4^s Σ_{k=0}^∞ [1/(4k +1)^s -1/(4k +3)^s ].

So for s=3, this becomes 4^3 Σ_{k=0}^∞ [1/(4k +1)^3 -1/(4k +3)^3 ] = 64 Σ_{k=0}^∞ [1/(4k +1)^3 -1/(4k +3)^3 ].

But this series is known as a Dirichlet beta function. The Dirichlet beta function is defined as β(s) = Σ_{k=0}^∞ (-1)^k / (2k +1)^s. However, our series is Σ_{k=0}^∞ [1/(4k +1)^3 -1/(4k +3)^3 ] = Σ_{k=0}^∞ [1/(4k)+1)^3 -1/(4k +3)^3 ].

But this is similar to β(3) but with a step of 4 instead of 2. Wait, but β(3) = Σ_{k=0}^∞ (-1)^k/(2k +1)^3. So our series is Σ_{k=0}^∞ [1/(4k +1)^3 -1/(4k +3)^3 ] = Σ_{m=0}^∞ [1/(4m +1)^3 -1/(4m +3)^3 ].

Let me make a substitution: let m = k. Then this is Σ_{m=0}^∞ [1/(4m +1)^3 -1/(4m +3)^3 ].

This can be written as Σ_{n=0}^∞ [1/(4n +1)^3 -1/(4n +3)^3 ].

But this is similar to the Dirichlet beta function but with a different step. Alternatively, note that this is the same as Σ_{n=0}^∞ [1/(4n +1)^3 + (-1)/(4n +3)^3 ].

If we consider the Dirichlet beta function β(s) = Σ_{n=0}^∞ (-1)^n/(2n +1)^s. If we split this into even and odd terms:

β(s) = Σ_{k=0}^∞ [1/(4k +1)^s -1/(4k +3)^s ].

Which is exactly our series when s=3. Therefore, β(3) = Σ_{k=0}^∞ [1/(4k +1)^3 -1/(4k +3)^3 ].

Therefore, our integral is 64 * β(3).

Wait, wait. Let me check:

We had ζ(3, 1/4) - ζ(3, 3/4) = 4^3 Σ_{k=0}^∞ [1/(4k +1)^3 -1/(4k +3)^3 ] = 64 β(3).

Therefore, the integral is equal to 64 β(3).

But the Dirichlet beta function β(3) is known to be π³/32. Wait, is that correct? Let me recall the value of β(3). The Dirichlet beta function at s=3 is approximately 0.96894614625936938048... and it's known that β(3) = π³/32. Let me verify:

Yes, indeed, β(3) = π³/32. Therefore, the integral becomes 64 * π³/32 = 2 π³.

Wait, that's a clean result! So the integral evaluates to 2 π³.

But let me confirm this step-by-step. So:

We had the original integral equal to ζ(3, 1/4) - ζ(3, 3/4) = 64 β(3) = 64*(π³/32) = 2 π³.

Yes, that seems correct. Therefore, the exact value of the integral is 2 π³.

Now, let's verify this with a numerical approximation. The numerical value of π is approximately 3.1415926536. Therefore, π³ ≈ 31.00627668. Multiply by 2: 62.01255336. Rounded to 10 decimal places, that's approximately 62.0125533603.

But let me check this with the series expansion. The Dirichlet beta function β(3) is indeed π³/32 ≈ 0.9689461463. Multiply by 64 gives 64 * 0.9689461463 ≈ 62.01255336, which matches.

Therefore, the exact answer is 2 π³, and the numerical approximation is approximately 62.0125533603.

But let me double-check the steps to ensure I didn't make a mistake. Let's recap:

1. Expanded the sinh terms into exponentials.
2. Split the integral into four terms, which after combining series, canceled out the first two terms.
3. The remaining terms were expressed as a difference of Hurwitz zeta functions at 1/4 and 3/4.
4. Recognized that this difference is related to the Dirichlet beta function β(3) = π³/32.
5. Multiplied by 64 to get 2 π³.

Yes, that seems correct. Therefore, the exact answer is 2π³, and the numerical value is approximately 62.0125533603.
</think>

{"answer": "2\\pi^3", "numerical_answer": "62.0125533603"}