<think>
Okay, so I need to compute the definite integral from 0 to 2.0 of x times cosine of 1.0 times the square root of x times (2.0 minus x) dx. Let me start by writing down the integral properly. The integral is ∫₀² x cos(√(x(2 - x))) dx. Hmm, the integrand is x multiplied by the cosine of a square root function. The square root part is √(x(2 - x)), which looks like a quadratic inside the square root. Maybe there's a substitution that can simplify this expression.

First, let me see if the expression under the square root can be rewritten. The term x(2 - x) is a quadratic that can be written as -x² + 2x. Completing the square for this quadratic: -x² + 2x = -(x² - 2x) = -(x² - 2x + 1 - 1) = -(x - 1)^2 + 1. So, √(x(2 - x)) = √[1 - (x - 1)^2]. That looks like the equation of a semicircle with radius 1 centered at (1, 0). Maybe a trigonometric substitution would work here. Let me try substituting (x - 1) = sinθ. Then, dx would be cosθ dθ, and the square root becomes √(1 - sin²θ) = cosθ. Let's check the limits. When x = 0, sinθ = -1, so θ = -π/2. When x = 2, sinθ = 1, so θ = π/2. So the integral becomes:

∫ from θ = -π/2 to θ = π/2 of (1 + sinθ) * cos(1.0 * cosθ) * cosθ dθ. Wait, let me make sure. The substitution is x = 1 + sinθ, so x = 1 + sinθ. Then, x in terms of θ is 1 + sinθ, and dx = cosθ dθ. The original integrand is x cos(√(x(2 - x))) dx. The square root part is √(x(2 - x)) = √[1 - (x - 1)^2] = √(1 - sin²θ) = cosθ. So the integrand becomes (1 + sinθ) * cos(cosθ) * cosθ dθ. So the integral is ∫_{-π/2}^{π/2} (1 + sinθ) cosθ cos(cosθ) dθ.

Hmm, that seems a bit complicated. Let me expand the terms. The integrand is (1 + sinθ) cosθ cos(cosθ) = [cosθ + sinθ cosθ] cos(cosθ). So splitting into two parts: cosθ cos(cosθ) + sinθ cosθ cos(cosθ). Let's split the integral into two parts: I1 = ∫ cosθ cos(cosθ) dθ and I2 = ∫ sinθ cosθ cos(cosθ) dθ. Maybe these can be simplified.

Starting with I2: the integral of sinθ cosθ cos(cosθ) dθ. Let me make a substitution here. Let u = cosθ. Then du = -sinθ dθ. So, sinθ dθ = -du. Then, the integral becomes ∫ u cos(u) (-du) = ∫ u cos(u) du. Wait, but there's a cosθ term as well. Wait, original I2 is ∫ sinθ * cosθ * cos(cosθ) dθ. So substituting u = cosθ, then du = -sinθ dθ, so sinθ dθ = -du. Then, cosθ is u. So the integral becomes ∫ u * u * cos(u) * (-du))?

Wait, let me re-express. The integral I2 is ∫ sinθ * cosθ * cos(cosθ) dθ. Let u = cosθ. Then du = -sinθ dθ. So sinθ dθ = -du. Then, cosθ is u, and cos(cosθ) is cos(u). So substituting, the integral becomes ∫ (u) * cos(u) * (-du). Wait, but the original integral is sinθ * cosθ * cos(cosθ) dθ = ∫ u * cos(u) * (-du). So that's -∫ u cos(u) du. Wait, but the limits when θ goes from -π/2 to π/2, u = cosθ. When θ = -π/2, u = cos(-π/2) = 0. When θ = π/2, u = cos(π/2) = 0. Wait, that's strange. So the limits for u would be from 0 to 0? Because cos(-π/2) is 0 and cos(π/2) is 0. So the integral I2 becomes -∫_{0}^{0} u cos(u) du, which is zero. Because the limits are the same. So I2 is zero. That's a relief. So the entire integral reduces to I1, which is ∫_{-π/2}^{π/2} cosθ cos(cosθ) dθ.

Now, let's focus on I1. The integrand is cosθ cos(cosθ). Let's note that the function cosθ cos(cosθ) is an even function. Because cos(-θ) = cosθ, and cos(cos(-θ)) = cos(cosθ). So the integrand is even. Therefore, the integral from -π/2 to π/2 is twice the integral from 0 to π/2. So I1 = 2 ∫₀}^{π/2} cosθ cos(cosθ) dθ.

Now, how to compute this integral. Let me consider substitution. Let’s set t = sinθ. Wait, maybe another substitution. Let me think. The integral is ∫ cosθ cos(cosθ) dθ. Let’s set u = sinθ. Then du = cosθ dθ. Wait, but then the integral becomes ∫ cos(cosθ) du. But cos(cosθ) is cos(√(1 - u²))? Wait, no. If u = sinθ, then cosθ = √(1 - u²). But that might complicate things. Alternatively, perhaps integrating by parts. Let me try integrating by parts. Let’s set u = cos(cosθ), dv = cosθ dθ. Then du = sin(cosθ) * sinθ dθ, and v = sinθ. So integration by parts gives uv - ∫ v du = sinθ cos(cosθ) - ∫ sinθ * sin(cosθ) * sinθ dθ. Hmm, that seems more complicated. Maybe not helpful.

Alternatively, perhaps expanding cos(cosθ) as a Taylor series. The Taylor series for cos(z) is Σ (-1)^n z^{2n}/(2n)!). So cos(cosθ) = Σ (-1)^n (cosθ)^{2n}/(2n)!). Then, multiplying by cosθ, the integrand becomes Σ (-1)^n (cosθ)^{2n + 1}/(2n)!). Then integrating term by term. But integrating (cosθ)^{2n + 1} from 0 to π/2. But integrating (cosθ)^{2n + 1} dθ can be done using reduction formulas or beta functions. However, this might lead to a series expression, which might not be helpful for an exact answer. Alternatively, perhaps there's a substitution that can be made.

Wait, let me check if the integral ∫ cosθ cos(cosθ) dθ can be expressed in terms of known functions. Let me consider substitution z = cosθ. Then dz = -sinθ dθ. But the integral is ∫ cosθ cos(cosθ) dθ. Let me write this as ∫ z cos(z) * (-dz)/sinθ. Wait, but sinθ = √(1 - z²). Hmm, this might not be helpful. Alternatively, perhaps substitution t = sinθ. Then dt = cosθ dθ. Then the integral becomes ∫ cos(√(1 - t²)) dt. Wait, but that's not helpful either. Hmm.

Alternatively, perhaps differentiation under the integral sign. Let me consider a parameter a in the integral. Let’s define I(a) = ∫ cosθ cos(a cosθ) dθ. Then, differentiating I(a) with respect to a, we get I’(a) = -∫ cosθ * sin(a cosθ) * cosθ dθ = -∫ cos²θ sin(a cosθ) dθ. Hmm, not sure if that helps. Alternatively, maybe integrating in terms of Bessel functions. Wait, the integral ∫ cosθ cos(cosθ) dθ might relate to Bessel functions. Let me recall that the integral representation of Bessel functions is J_n(x) = (1/π) ∫₀^π cos(nθ - x sinθ) dθ. But I'm not sure if that's directly applicable here.

Alternatively, perhaps using substitution u = cosθ. Then, when θ goes from 0 to π/2, u goes from 1 to 0. So the integral I1 is 2 ∫₀^{π/2} cosθ cos(cosθ) dθ = 2 ∫₀¹ cos(u) * (-du)/sqrt(1 - u²). Wait, no. Wait, if u = cosθ, then when θ increases from 0 to π/2, u decreases from 1 to 0. So du = -sinθ dθ. But we have cosθ dθ. Let me see. The integral is ∫ cosθ cos(cosθ) dθ. If u = cosθ, then du = -sinθ dθ. So sinθ dθ = -du. But we have cosθ dθ. Let me express cosθ dθ in terms of u. Hmm, cosθ dθ = (du)/(-sinθ). But sinθ = sqrt(1 - u²). So cosθ dθ = -du / sqrt(1 - u²). Therefore, the integral becomes ∫ u cos(u) * (-du)/sqrt(1 - u²) from u=1 to u=0. Changing the limits, it becomes ∫₁⁰ [ -u cos(u) / sqrt(1 - u²) ] du = ∫₀¹ [ u cos(u) / sqrt(1 - u²) ] du. So I1 = 2 ∫₀¹ [ u cos(u) / sqrt(1 - u²) ] du. Hmm, this seems more complicated. Maybe not helpful.

Alternatively, perhaps numerical integration is the way to go, but the problem says to compute the integral analytically first. Wait, the problem says to compute the integral analytically to obtain the exact answer. So maybe there's a trick here. Let me think again.

Wait, going back to the original substitution. The integral after substitution became I1 = 2 ∫₀^{π/2} cosθ cos(cosθ) dθ. Let me consider expanding cos(cosθ) into its Fourier series or Taylor series. The Taylor series expansion of cos(cosθ) is Σ_{n=0}^∞ (-1)^n (cosθ)^{2n} / (2n)!). Then, multiplying by cosθ, the integrand becomes Σ_{n=0}^∞ (-1)^n (cosθ)^{2n + 1} / (2n)!). Then, integrating term by term:

I1 = 2 Σ_{n=0}^∞ [ (-1)^n / (2n)! ) ∫₀^{π/2} (cosθ)^{2n + 1} dθ ]

The integral ∫₀^{π/2} (cosθ)^{2n + 1} dθ can be evaluated using the beta function. Recall that ∫₀^{π/2} (cosθ)^k dθ = (sqrt(π)/2) Γ((k + 1)/2) / Γ((k + 2)/2). For k = 2n + 1, this becomes (sqrt(π)/2) Γ(n + 1) / Γ(n + 3/2). And Γ(n + 1) = n! and Γ(n + 3/2) = (sqrt(π)/2^{2n + 1}) (2n + 1)! ) / n! ). Wait, maybe I should recall the formula for the beta function. The integral ∫₀^{π/2} sin^m θ cos^n θ dθ = (1/2) B((m + 1)/2, (n + 1)/2). For our case, m = 0, n = 2n + 1. So it's (1/2) B(1/2, n + 1). The beta function B(a, b) = Γ(a)Γ(b)/Γ(a + b). So this becomes (1/2) Γ(1/2)Γ(n + 1)/Γ(n + 3/2). Since Γ(1/2) = sqrt(π), so the integral is (sqrt(π)/2) Γ(n + 1)/Γ(n + 3/2).

Now, Γ(n + 3/2) can be written as (n + 1/2) Γ(n + 1/2). And Γ(n + 1/2) = (sqrt(π)/2^{2n}) (2n)! ) / n! ). Wait, let me recall that Γ(n + 1/2) = (2n)! sqrt(π) ) / (4^n n! ). So Γ(n + 3/2) = (n + 1/2) Γ(n + 1/2) = (n + 1/2) * (2n)! sqrt(π) ) / (4^n n! ). Therefore, Γ(n + 1)/Γ(n + 3/2) = n! / [ (n + 1/2) * (2n)! sqrt(π) / (4^n n! ) ) ] = n! * 4^n n! / [ (2n)! sqrt(π) (n + 1/2) ) ].

Hmm, this is getting complicated. Let me see if there's a simpler expression. Alternatively, using the duplication formula for Gamma functions. But maybe there's a better way. Let me compute the first few terms to see if a pattern emerges. For n=0: ∫₀^{π/2} cosθ dθ = 1. For n=0, the formula gives (sqrt(π)/2) Γ(1)/Γ(3/2). Γ(1) = 1, Γ(3/2) = (1/2) sqrt(π). So (sqrt(π)/2) * 1 / ( (1/2) sqrt(π) ) ) = (sqrt(π)/2) * 2 / sqrt(π) ) = 1. Correct. For n=1: ∫ cos^3θ dθ from 0 to π/2. The integral is 2/3. Let's check the formula: (sqrt(π)/2) Γ(2)/Γ(5/2). Γ(2) = 1! = 1. Γ(5/2) = (3/2)(1/2)sqrt(π) = (3/4)sqrt(π). So (sqrt(π)/2) * 1 / ( (3/4)sqrt(π) ) ) = (sqrt(π)/2) * 4/(3 sqrt(π)) ) = 2/3. Correct. So the formula works.

Therefore, the integral ∫₀^{π/2} (cosθ)^{2n + 1} dθ = (sqrt(π)/2) Γ(n + 1)/Γ(n + 3/2). Therefore, substituting back into I1:

I1 = 2 Σ_{n=0}^∞ [ (-1)^n / (2n)! ) * (sqrt(π)/2) Γ(n + 1)/Γ(n + 3/2) ) ]

Simplify this expression:

I1 = sqrt(π) Σ_{n=0}^∞ [ (-1)^n / (2n)! ) * Γ(n + 1)/Γ(n + 3/2) ) ]

But Γ(n + 1) = n! and Γ(n + 3/2) = (sqrt(π)/2^{2n + 1}) (2n + 2)! ) / (n + 1)! )? Wait, maybe I should use the expression for Γ(n + 3/2) in terms of factorials. As I mentioned earlier, Γ(n + 3/2) = (2n + 1)! ) sqrt(π) / (4^{n + 1/2} n! ) ). Wait, let me recall that Γ(n + 1/2) = (2n)! sqrt(π) ) / (4^n n! ). Therefore, Γ(n + 3/2) = Γ( (n + 1) + 1/2 ) = (2(n + 1) - 1)! sqrt(π) ) / (4^{n + 1} (n + 1)! ) )? Wait, no. Let me check for n=0: Γ(3/2) = (1/2)sqrt(π). Using the formula Γ(n + 1/2) = (2n)! sqrt(π) ) / (4^n n! ). For n=1: Γ(3/2) = (2*1)! sqrt(π) ) / (4^1 1! ) = 2 sqrt(π)/4 = sqrt(π)/2. Which is correct. So Γ(n + 3/2) = Γ( (n + 1) + 1/2 ) = (2(n + 1) - 1)! sqrt(π) ) / (4^{n + 1} (n + 1)! ) )? Wait, no. Wait, for Γ(m + 1/2), m = n + 1. So Γ(m + 1/2) = (2m)! sqrt(π) ) / (4^m m! ). So Γ(n + 3/2) = Γ( (n + 1) + 1/2 ) = (2(n + 1))! sqrt(π) ) / (4^{n + 1} (n + 1)! ) ). Therefore, Γ(n + 3/2) = (2n + 2)! sqrt(π) ) / (4^{n + 1} (n + 1)! ) ). Therefore, Γ(n + 1)/Γ(n + 3/2) = n! / [ (2n + 2)! sqrt(π) / (4^{n + 1} (n + 1)! ) ) ] = n! * 4^{n + 1} (n + 1)! ) / [ (2n + 2)! sqrt(π) ) ].

Simplify this:

4^{n + 1} = 4 * 4^n. The denominator (2n + 2)! = (2n + 2)(2n + 1)(2n)! ). So:

Γ(n + 1)/Γ(n + 3/2) = [n! * 4 * 4^n (n + 1)! ] / [ (2n + 2)(2n + 1)(2n)! ) sqrt(π) ) ]

But (n + 1)! = (n + 1) n! So:

= [n! * 4 * 4^n (n + 1) n! ] / [ (2n + 2)(2n + 1)(2n)! ) sqrt(π) ) ]

Simplify numerator and denominator:

Numerator: 4 * 4^n (n + 1) (n! )^2

Denominator: (2n + 2)(2n + 1)(2n)! sqrt(π)

But (2n + 2) = 2(n + 1), so denominator becomes 2(n + 1)(2n + 1)(2n)! sqrt(π)

So:

Γ(n + 1)/Γ(n + 3/2) = [4^{n + 1} (n + 1) (n! )^2 ] / [2(n + 1)(2n + 1)(2n)! sqrt(π) ) ]

Cancel (n + 1) terms:

= [4^{n + 1} (n! )^2 ] / [2(2n + 1)(2n)! sqrt(π) ) ]

Note that 4^{n + 1} = 2^{2n + 2}, and 2(2n + 1) = 2(2n + 1). Also, (2n)! = (2n)(2n - 1)...1, and (n! )^2 = n! n!.

But there's a formula for (2n)! = 2^{2n} n! (n)! / (sqrt(π n) ) )? Wait, no. Wait, using the relation between binomial coefficients and factorials. Alternatively, perhaps using the term (n! )^2 / (2n)! ) = 1 / ( (2n choose n) ). But I'm not sure. Let me see:

Alternatively, note that (2n)! = 2^n n! product_{k=1}^n (2k - 1). So (2n)! = 2^n n! (1 * 3 * 5 * ... (2n - 1)). Therefore, (n! )^2 / (2n)! ) = n! / (2^n (1 * 3 * 5 * ... * (2n - 1)) ). Hmm, not sure.

But let's substitute back into the expression:

Γ(n + 1)/Γ(n + 3/2) = [4^{n + 1} (n! )^2 ] / [2(2n + 1)(2n)! sqrt(π) ) ]

= [4 * 4^n (n! )^2 ] / [2(2n + 1)(2n)! sqrt(π) ) ]

= [2 * 4^n (n! )^2 ] / [ (2n + 1)(2n)! sqrt(π) ) ]

Now, substituting back into I1:

I1 = sqrt(π) Σ_{n=0}^∞ [ (-1)^n / (2n)! ) * [2 * 4^n (n! )^2 ] / [ (2n + 1)(2n)! sqrt(π) ) ] ]

Simplify:

The sqrt(π) cancels with the denominator's sqrt(π):

I1 = Σ_{n=0}^∞ [ (-1)^n / (2n)! ) * [2 * 4^n (n! )^2 ] / [ (2n + 1)(2n)! ) ] ]

= 2 Σ_{n=0}^∞ [ (-1)^n 4^n (n! )^2 / ( (2n)! )^2 (2n + 1) ) ]

Hmm, this seems quite complicated. Let me see if this series can be recognized. Let's write it as:

I1 = 2 Σ_{n=0}^∞ [ (-1)^n (4^n (n! )^2 ) / ( (2n)! )^2 (2n + 1) ) ]

Alternatively, note that 4^n (n! )^2 / (2n)! )^2 = [ (2^n n! ) / (2n)! ) ]^2. But 2^n n! = 2*4*6*...*2n, and (2n)! = 1*2*3*...*2n. So 2^n n! / (2n)! ) = (2*4*6*...*2n) / (1*2*3*...*2n) ) = 1 / (1*3*5*...*(2n - 1)) ). So [2^n n! / (2n)! )]^2 = 1 / [ (1*3*5*...*(2n - 1))^2 ].

But I'm not sure if this helps. Alternatively, perhaps this series is related to the Taylor series of arcsin or something similar. Let me recall that the Taylor series for arcsin(x) is Σ_{n=0}^∞ ( (2n)! ) / (4^n (n! )^2 (2n + 1) ) ) x^{2n + 1}. So if we compare, the coefficients here are similar but with (-1)^n and different factors. Let's see:

The coefficient in arcsin(x) is (2n)! / (4^n (n! )^2 (2n + 1) ). In our series, the coefficient is (-1)^n 4^n (n! )^2 / ( (2n)! )^2 (2n + 1) ). Not quite the same. Alternatively, perhaps integrating term by term.

Alternatively, maybe there's a better substitution. Let me go back to the original integral. The integral can be written as ∫₀² x cos(√(x(2 - x))) dx. Let me try another substitution. Let’s set t = x - 1. Then, when x=0, t=-1; when x=2, t=1. The integral becomes ∫_{-1}^{1} (t + 1) cos(√{(t + 1)(1 - t)}) dt. The square root simplifies to √(1 - t²). So the integral becomes ∫_{-1}^{1} (t + 1) cos(√(1 - t²)) dt. This can be split into two integrals: ∫_{-1}^{1} t cos(√(1 - t²)) dt + ∫_{-1}^{1} cos(√(1 - t²)) dt.

The first integral, ∫_{-1}^{1} t cos(√(1 - t²)) dt, is an integral of an odd function over symmetric limits. Since t is odd and cos(√(1 - t²)) is even (since √(1 - t²) is even), the product t * cos(...) is odd. Therefore, the integral from -1 to 1 is zero. So the integral reduces to ∫_{-1}^{1} cos(√(1 - t²)) dt. Which is twice the integral from 0 to 1 of cos(√(1 - t²)) dt. So now, the problem reduces to evaluating 2 ∫₀¹ cos(√(1 - t²)) dt. Let me make a substitution here. Let u = √(1 - t²). Then, u² = 1 - t², so t = √(1 - u²). Then, dt = (-u du)/√(1 - u²). Wait, but when t goes from 0 to 1, u goes from 1 to 0. So the integral becomes:

2 ∫_{u=1}^{u=0} cos(u) * (-u du)/√(1 - u²) ) = 2 ∫₀¹ [ u cos(u) / √(1 - u²) ] du.

Wait, this is the same integral as before. So we end up back at the same point. Hmm. So maybe this approach isn't helping. Let me think differently.

Wait, perhaps switching to polar coordinates. Since the integral involves √(1 - t²), which is reminiscent of a circle. Let me set t = sinφ, where φ ranges from 0 to π/2. Then, dt = cosφ dφ, and √(1 - t²) = cosφ. So the integral becomes ∫₀^{π/2} cos(cosφ) cosφ dφ. Wait, but this is the same as the previous integral I1. So we're back to where we were before. It seems like we're going in circles.

Alternatively, perhaps differentiating under the integral sign. Let’s consider the integral I(a) = ∫₀² x cos(a√(x(2 - x))) dx. Then, we need to find I(1.0). Let's compute I(a)=

Differentiating I(a) with respect to a:

I’(a) = -∫₀² x √(x(2 - x)) sin(a√(x(2 - x))) dx.

This seems more complicated. Alternatively, maybe integrating by parts. Let’s try integrating the original integral by parts. Let u = x, dv = cos(√(x(2 - x))) dx. Then, du = dx, and v = ∫ cos(√(x(2 - x))) dx. But integrating dv is not straightforward. Alternatively, perhaps another choice. Let’s set u = something that differentiates to x, but not sure.

Alternatively, let me consider the original substitution again. After substitution x = 1 + sinθ, the integral became I1 = 2 ∫₀^{π/2} cosθ cos(cosθ) dθ. Let me check if this integral can be expressed in terms of known special functions. The integral ∫ cosθ cos(cosθ) dθ from 0 to π/2. Let me look up integral tables or properties.

Upon checking, I recall that integrals of the form ∫ cos(a cosθ) dθ are related to Bessel functions. Specifically, the zeroth Bessel function J₀(a) is given by (1/π) ∫₀^π cos(a cosθ) dθ. So, ∫₀^π cos(a cosθ) dθ = π J₀(a). Similarly, ∫₀^{π/2} cos(a cosθ) dθ = (π/2) J₀(a) + something? Wait, not sure. Let me verify.

The standard integral representation for J₀(a) is J₀(a) = (1/π) ∫₀^π cos(a sinθ) dθ. Wait, there are different forms. Let me check:

Yes, J₀(a) = (1/π) ∫₀^π cos(a sinθ) dθ. Also, J₀(a) = (1/2π) ∫₀^{2π} e^{i a sinθ} dθ. So, the integral ∫₀^π cos(a cosθ) dθ might not directly relate to J₀(a), but perhaps there's a relation.

Alternatively, using substitution φ = π/2 - θ. Then, cosθ = sinφ. So ∫₀^{π/2} cos(a cosθ) dθ = ∫₀^{π/2} cos(a sinφ) dφ. Which is similar to the integral for J₀(a). Since J₀(a) = (1/π) ∫₀^π cos(a sinθ) dθ, then ∫₀^π cos(a sinθ) dθ = π J₀(a). Therefore, ∫₀^{π/2} cos(a sinθ) dθ = (1/2) ∫₀^π cos(a sinθ) dθ = (π/2) J₀(a). So, ∫₀^{π/2} cos(a cosθ) dθ = ∫₀^{π/2} cos(a sinφ) dφ = (π/2) J₀(a). Therefore, ∫₀^{π/2} cosθ cos(cosθ) dθ = ?

Wait, but our integral is ∫₀^{π/2} cosθ cos(cosθ) dθ, which is different from ∫ cos(a cosθ) dθ. However, perhaps differentiating with respect to a. Let’s consider I(a) = ∫₀^{π/2} cos(a cosθ) dθ. Then, I’(a) = -∫₀^{π/2} sin(a cosθ) cosθ dθ. But our integral is ∫ cosθ cos(cosθ) dθ, which is I’(1) with a negative sign. Wait, let's see:

If I(a) = ∫₀^{π/2} cos(a cosθ) dθ, then I’(a) = -∫₀^{π/2} sin(a cosθ) cosθ dθ. So, our integral is ∫₀^{π/2} cosθ cos(cosθ) dθ = -I’(1). But we know that I(a) = (π/2) J₀(a). Therefore, I’(a) = (π/2) J₀(a). The derivative of J₀(a) is -J₁(a). So, I’(a) = (π/2) (-J₁(a)). Therefore, our integral is -I’(1) = (π/2) J₁(1).

Therefore, I1 = 2 * (π/2) J₁(1) = π J₁(1). So the original integral is equal to π times the Bessel function of the first kind of order 1 evaluated at 1. Therefore, the exact answer is π J₁(1).

But the problem asks for the exact answer. So, in terms of Bessel functions, the integral ∫₀² x cos(√(x(2 - x))) dx = π J₁(1). Therefore, the exact answer is π J_1(1). Now, to write this in LaTeX, it would be \pi J_1(1). However, sometimes Bessel functions are written with a subscript, so J_1(1). 

Now, for the numerical approximation. The value of J₁(1) is a known constant. The Bessel function J₁(1) is approximately 0.4400505857. So multiplying by π gives π * 0.4400505857 ≈ 1.382459904. Rounded to 10 decimal places, this is approximately 1.3824599043. Let me verify this value.

Checking a table or calculator for J₁(1): The Bessel function J₁(1) is indeed approximately 0.4400505857. Therefore, π times that is approximately 3.1415926536 * 0.4400505857 ≈ 1.382459904. Rounded to 10 decimal places, 1.3824599043. So the numerical approximation is 1.3824599043.

Therefore, the final answer is {"answer": "\pi J_1(1)", "numerical_answer": 1.3824599043}.
</think>

{"answer": "\\pi J_1(1)", "numerical_answer": "1.3824599043"}