Given:
\[
I = \int_{0}^{1} \arctan(\sqrt{x(1-x)}) \, dx
\]

Let's proceed step by step.

---

**Step 1: Substitution**

Let’s use the substitution: \( x = \sin^2\theta \), so that \( dx = 2\sin\theta\cos\theta\,d\theta = \sin2\theta\,d\theta \) and when \( x = 0 \), \( \theta = 0 \); when \( x = 1 \), \( \theta = \frac{\pi}{2} \).

Also,
\[
x(1-x) = \sin^2\theta (1 - \sin^2\theta) = \sin^2\theta \cos^2\theta = \frac{1}{4}\sin^2(2\theta)
\]
So,
\[
\sqrt{x(1-x)} = \frac{1}{2} |\sin(2\theta)|
\]
But since \( \theta \in [0, \frac{\pi}{2}] \), \(\sin(2\theta) \geq 0 \).

Thus:
\[
I = \int_{x=0}^{x=1} \arctan( \sqrt{ x (1-x) } ) dx = \int_{\theta=0}^{\theta=\frac{\pi}{2}} \arctan\left( \frac{1}{2} \sin 2\theta \right) \cdot \sin 2\theta\, d\theta
\]

---

**Step 2: New substitution**

Let’s set \( u = \sin 2\theta \), \( du = 2\cos 2\theta\,d\theta \). However, let's focus on integrating by parts.

Let:
- \( f(\theta) = \arctan\left( \frac{1}{2} \sin 2\theta \right) \)
- \( g'(\theta) = \sin 2\theta \)

Then \( g(\theta) = -\frac{1}{2}\cos 2\theta \).

Applying integration by parts:
\[
I = \left. f(\theta) g(\theta) \right|_0^{\pi/2} - \int_0^{\pi/2} f'(\theta) g(\theta) d\theta
\]

First,
\[
f(\theta) = \arctan\left( \frac{1}{2} \sin 2\theta \right), \quad g(\theta) = -\frac{1}{2} \cos 2\theta
\]
So,
\[
I = -\frac{1}{2} \left. \arctan\left( \frac{1}{2} \sin 2\theta \right) \cos 2\theta \right|_0^{\pi/2}
+ \frac{1}{2} \int_0^{\pi/2} \cos 2\theta \cdot \frac{d}{d\theta}\left[\arctan\left( \frac{1}{2} \sin 2\theta \right)\right] d\theta
\]

Let’s compute the boundary term first:
- At \(\theta = 0\): \(\sin 0 = 0\), so \(\arctan(0) = 0\), \(\cos 0 = 1\).
- At \(\theta = \frac{\pi}{2}\): \(\sin(\pi) = 0\), so \(\arctan(0) = 0\), \(\cos(\pi) = -1\).

Boundary term:
\[
-\frac{1}{2} \left[ 0 \cdot (-1) - 0 \cdot 1 \right] = 0
\]

The integral itself is:
\[
I = \frac{1}{2} \int_0^{\pi/2} \cos 2\theta \cdot
\frac{d}{d\theta} \arctan \left( \frac{1}{2} \sin 2\theta \right) d\theta
\]

Compute the derivative:
\[
\frac{d}{d\theta} \arctan \left( \frac{1}{2} \sin 2\theta \right)
= \frac{1}{1 + \left( \frac{1}{2} \sin 2\theta \right)^2 }
\cdot \frac{d}{d\theta} \left( \frac{1}{2} \sin 2\theta \right )
= \frac{1}{1 + \frac{1}{4} \sin^2 2\theta } \cdot \cos 2\theta
\]

Therefore:
\[
I = \frac{1}{2} \int_0^{\pi/2} \cos 2\theta \cdot
\frac{\cos 2\theta}{1 + \frac{1}{4} \sin^2 2\theta} d\theta
= \frac{1}{2} \int_0^{\pi/2} \frac{\cos^2 2\theta}{1 + \frac{1}{4} \sin^2 2\theta} d\theta
\]

---

Now, recall \( \cos^2 2\theta = 1 - \sin^2 2\theta \), so:

\[
I = \frac{1}{2} \int_0^{\pi/2} 
\frac{1 - \sin^2 2\theta }{ 1 + \frac{1}{4} \sin^2 2\theta }
d\theta
\]

Let’s split the integral:

\[
I = \frac{1}{2} \int_0^{\pi/2} \frac{1}{ 1 + \frac{1}{4} \sin^2 2\theta } d\theta
- \frac{1}{2} \int_0^{\pi/2} \frac{ \sin^2 2\theta }{ 1 + \frac{1}{4} \sin^2 2\theta } d\theta
\]

Let’s note that:

\[
\frac{ \sin^2 2\theta }{ 1 + \frac{1}{4} \sin^2 2\theta } =
\frac{ 4 u^2 }{ 4 + u^2 }, \quad \text{where} \ u = \sin 2\theta
\]
So that:
\[
\frac{1}{ 1 + \frac{1}{4} \sin^2 2\theta } = 
\frac{ 4 }{ 4 + \sin^2 2\theta }
\]

Therefore,

\[
I = \frac{1}{2} \int_0^{\pi/2} \frac{4}{4+\sin^2 2\theta} d\theta
  - \frac{1}{2} \int_0^{\pi/2} \frac{4 \sin^2 2\theta}{4+\sin^2 2\theta} d\theta
\]

But notice:
\[
\frac{4 \sin^2 2\theta }{4+\sin^2 2\theta } = 4 - \frac{16}{4+\sin^2 2\theta }
\]

So:

\[
I = \frac{1}{2} \int_0^{\pi/2} \frac{4}{4+\sin^2 2\theta} d\theta 
- \frac{1}{2} \left( 4 \int_0^{\pi/2} d\theta - \int_0^{\pi/2} \frac{16}{4+\sin^2 2\theta } d\theta \right )
\]

\[
= \frac{1}{2} \int_0^{\pi/2} \frac{4}{4+\sin^2 2\theta} d\theta 
- 2 \pi + \frac{1}{2} \int_0^{\pi/2} \frac{16}{4+\sin^2 2\theta } d\theta
\]

\[
= \frac{1}{2} \int_0^{\pi/2} \left ( \frac{4}{4+\sin^2 2\theta} + \frac{16}{4+\sin^2 2\theta} \right ) d\theta - 2 \cdot \frac{\pi}{2}
\]
\[
= \frac{1}{2} \int_0^{\pi/2} \frac{20}{4+\sin^2 2\theta} d\theta - \pi
\]

Thus,
\[
I = 10 \int_0^{\pi/2} \frac{d\theta}{4+\sin^2 2\theta} - \pi
\]

Let’s let \( \phi = 2\theta \implies \theta \in [0, \frac{\pi}{2}] \implies \phi \in [0, \pi] \), and \( d\phi = 2 d\theta \).

So:
\[
\int_0^{\pi/2} \frac{d\theta}{4+\sin^2 2\theta}
= \int_{\theta=0}^{\theta=\pi/2} \frac{d\theta}{4+\sin^2 2\theta}
= \frac{1}{2} \int_{\phi=0}^{\phi=\pi} \frac{d\phi}{4+\sin^2 \phi}
\]

So finally:
\[
I = 10 \cdot \frac{1}{2} \int_0^{\pi} \frac{d\phi}{4+\sin^2 \phi} - \pi
= 5 \int_0^{\pi} \frac{d\phi}{4+\sin^2 \phi} - \pi
\]

---

**Now, close the analytic step:**

The integral is:
\[
\boxed{
I = 5 \int_0^{\pi} \frac{d\phi}{4+\sin^2 \phi} - \pi
}
\]

This is the exact answer in terms of elementary functions and a definite integral. 

Let’s further evaluate the remaining integral in closed form, if possible.

Let’s recall for constants \( a^2 > b^2 > 0 \):

\[
\int_0^\pi \frac{d\phi}{a + b\,\sin\phi}
= \frac{\pi}{\sqrt{a^2-b^2}}
\]

But in our case, denominator is \(4 + \sin^2\phi\), not \(a+b\sin\phi\).

Let’s try to express this integral.

Alternatively, recall
\[
\int_0^{\pi}\frac{d\phi}{A+B\cos\phi} = \frac{\pi}{\sqrt{A^2-B^2}}
\]
But our denominator is \(4+\sin^2\phi\).

Let's write \( \sin^2\phi = 1 - \cos^2\phi \), but perhaps it's better to use the standard approach.

Let’s use the Weierstrass substitution, \( t = \tan(\phi/2) \):

\[
\sin \phi = \frac{2t}{1+t^2}, \quad
d\phi = \frac{2dt}{1+t^2}, \quad
t \in [0, +\infty]
\]

So,
\(
\sin^2 \phi = \frac{4 t^2}{(1 + t^2)^2 }
\)
and
\(
4 + \sin^2\phi = 4 + \frac{4t^2}{(1 + t^2)^2 }
= \frac{4(1 + t^2)^2 + 4t^2}{ (1 + t^2)^2 }
= \frac{4(1 + t^2)^2 + 4t^2}{(1 + t^2)^2 }
\)

Let’s expand numerator:

\[
4(1 + t^2)^2 + 4t^2 = 4(1 + 2t^2 + t^4) + 4t^2 = 4 + 8t^2 + 4t^4 + 4t^2 = 4 + 12t^2 + 4t^4 = 4(1 + 3t^2 + t^4)
\]

So:
\[
4 + \sin^2\phi = \frac{4(1 + 3t^2 + t^4)}{(1 + t^2)^2}
\]

Now, \( d\phi = \frac{2dt}{1+t^2 } \):

Therefore,
\[
\int_0^{\pi} \frac{d\phi}{4 + \sin^2\phi} =
\int_{t=0}^{t=+\infty} \frac{2 dt}{1+t^2} \cdot \frac{ (1 + t^2 )^2 }{4(1 + 3 t^2 + t^4 ) }
= \frac{1}{2} \int_{0}^{\infty} \frac{ (1 + t^2 ) dt }{ 1 + 3 t^2 + t^4 }
\]

Expand numerator inside:
\[
(1 + t^2)^2 / (1 + 3 t^2 + t^4 ) = (1 + 2 t^2 + t^4 ) / (1 + 3 t^2 + t^4 )
\]

So,
\[
\int_0^{\pi} \frac{d\phi}{4+\sin^2\phi}
= \frac{1}{2} \int_0^\infty \frac{1 + 2 t^2 + t^4 }{ 1 + 3 t^2 + t^4 } dt
= \frac{1}{2} \int_0^\infty \frac{ dt }{ 1 + 3 t^2 + t^4 }
+ \int_0^\infty \frac{ t^2 dt }{ 1 + 3 t^2 + t^4 }
\]

But 
\[
\frac{1 + 2 t^2 + t^4 }{ 1 + 3 t^2 + t^4 } = 1 - \frac{ t^2 }{ 1 + 3 t^2 + t^4 }
\]

Therefore,
\[
\int_0^{\pi} \frac{d\phi}{4+\sin^2\phi}
= \frac{1}{2} \left [ \int_0^\infty dt - \int_0^\infty \frac{ t^2 dt }{ 1 + 3 t^2 + t^4 } \right ]
\]

But the first integral diverges, indicating this route is not helpful for a simple closed form.

Let us recall a table integral (see Gradshteyn & Ryzhik 3.621):

\[
\int_0^\pi \frac{d\phi}{p + q \sin^2\phi}
= \frac{\pi}{ \sqrt{p(p+q)} }
\]
See 3.621.3 for \( p>0 \), \( p+q>0 \).

For us, \( p=4,\ q=1\):

\(
p = 4,\quad q=1 \implies p+q = 5
\)

Therefore,
\[
\int_0^\pi \frac{d\phi}{4 + \sin^2 \phi }
= \frac{\pi}{ \sqrt{4 \times 5 } }
= \frac{\pi}{2 \sqrt{5} }
\]

Therefore our original answer is:

\[
I = 5 \cdot \frac{\pi}{2\sqrt{5}} - \pi = \frac{5\pi}{2\sqrt{5}} - \pi
= \pi\left( \frac{5}{2\sqrt{5}} - 1 \right)
= \pi\left( \frac{5-2\sqrt{5}}{2\sqrt{5}} \right )
\]

If we rationalize the denominator:
\[
\frac{5-2\sqrt{5}}{2\sqrt{5}} \cdot \frac{\sqrt{5}}{\sqrt{5}} = \frac{5\sqrt{5}-2 \times 5}{2 \times 5}
= \frac{5\sqrt{5} - 10}{10}
\]

Thus,
\[
\boxed{
I = \pi \cdot \frac{5\sqrt{5} - 10}{10}
}
\]

---

**Step 3: Numerical Approximation**

Compute \( 5\sqrt{5}-10 \):

\( \sqrt{5} \approx 2.2360679775 \)

\( 5\sqrt{5} \approx 11.1803398875 \)

\( 11.1803398875 - 10 = 1.1803398875 \)

Divided by 10: \( 0.11803398875 \)

So,

\[
I = \pi \times 0.11803398875 \approx 0.3708118206
\]
(using \( \pi \approx 3.1415926536 \))

---

**Final JSON output:**
```json
{"answer": "\\pi \\cdot \\frac{5\\sqrt{5} - 10}{10}", "numerical_answer": "0.3708118206"}
```