
To solve the definite integral \(\int_0^1 \frac{x-1}{(x+1)\ln x} \, dx\), we proceed as follows:

### Step 1: Introduce a Parameter and Differentiate
Define \(I(a) = \int_0^1 \frac{x^a - 1}{(x+1)\ln x} \, dx\). The original integral is \(I(1)\). Differentiating \(I(a)\) with respect to \(a\) (using Leibnizâ€™s rule for differentiation under the integral sign), we get:
\[
I'(a) = \int_0^1 \frac{x^a}{x+1} \, dx.
\]

### Step 2: Evaluate \(I'(a)\)
The integral \(I'(a)\) can be expressed using the digamma function \(\psi(z)\), which satisfies \(\int_0^1 \frac{x^a}{x+1} \, dx = \frac{1}{2} \left( \psi\left( \frac{a+2}{2} \right) - \psi\left( \frac{a+1}{2} \right) \right)\). This result follows from properties of the digamma function and its relation to alternating series.

### Step 3: Integrate \(I'(a)\) to Find \(I(a)\)
Integrate \(I'(a)\) from \(a=0\) to \(a=1\) to recover \(I(1)\). Using \(\int \psi(z) \, dz = \ln \Gamma(z) + C\) (where \(\Gamma(z)\) is the gamma function), we find:
\[
I(a) = \frac{1}{2} \left( \ln \Gamma\left( \frac{a+2}{2} \right) - \ln \Gamma\left( \frac{a+1}{2} \right) \right) + \frac{1}{4} \ln \pi.
\]

### Step 4: Substitute \(a=1\)
For \(a=1\), substitute into the expression for \(I(a)\):
\[
I(1) = \frac{1}{2} \left( \ln \Gamma\left( \frac{3}{2} \right) - \ln \Gamma(1) \right) + \frac{1}{4} \ln \pi.
\]
Since \(\Gamma(1) = 1\) and \(\Gamma\left( \frac{3}{2} \right) = \frac{\sqrt{\pi}}{2}\), we simplify:
\[
I(1) = \frac{1}{2} \ln\left( \frac{\sqrt{\pi}/2}{1} \right) + \frac{1}{4} \ln \pi = \frac{1}{2} \ln\left( \frac{\pi}{2} \right).
\]

### Numerical Approximation
The exact result is \(\frac{1}{2} \ln\left( \frac{\pi}{2} \right)\). Numerically, this approximates to \(0.2257913526\) (rounded to 10 decimal places).

{"answer": "\\frac{1}{2} \\ln\\left(\\frac{\\pi}{2}\\right)", "numerical_answer": "0.2257913526"}