We wish to evaluate

  I = ∫₁∞ (x² – 1²)^(2 – ½) e^(–(0.5)² x²) H₍₂×2+1₎(0.5x) dx.

A first step is to simplify the notation. Note that

  2 – ½ = 3/2  and  (0.5)² = 0.25.

Also, the Hermite polynomial is given by
  H₅(0.5x).
(Here Hₙ denotes the (physicists’) Hermite polynomial.) Recall that
  H₅(z) = 32z⁵ – 160z³ + 120z.
Hence
  H₅(0.5x) = 32 (0.5x)⁵ – 160 (0.5x)³ + 120 (0.5x)
          = 32 (x⁵/32) – 160 (x³/8) + 60x
          = x⁵ – 20x³ + 60x.

Thus our integral becomes

  I = ∫₁∞ (x² – 1)^(3/2) e^(–0.25 x²) [x⁵ – 20x³ + 60x] dx.

Step 1. Change of Variable

It will be convenient to change the variable. Write:
  u = x²  ⇒ du = 2x dx  or dx = du/(2x).
Since x = √u, we have
  (x² – 1)^(3/2) = (u – 1)^(3/2)
and
  x⁵ – 20x³ + 60x = u^(5/2) – 20 u^(3/2) + 60 u^(1/2).

Substitute these into the integral:
  I = ∫ from u=1 to ∞ [ (u – 1)^(3/2) e^(–0.25 u) {u^(5/2) – 20 u^(3/2) + 60 u^(1/2)} ] · [du/(2√u) ].
Notice that u^(5/2)/√u = u², u^(3/2)/√u = u, and u^(1/2)/√u = 1. Hence
  I = 1/2 ∫₁∞ e^(–0.25 u) (u – 1)^(3/2) (u² – 20u + 60) du.

Now, make a further substitution:
  t = u – 1  ⇒ u = t + 1  and du = dt.
When u = 1, t = 0; when u = ∞, t = ∞. Also
  (u – 1)^(3/2) becomes t^(3/2),
and the polynomial becomes
  (t+1)² – 20(t+1) + 60.
Compute:
  (t+1)² = t² + 2t + 1,
so
  t² + 2t + 1 – 20t – 20 + 60 = t² – 18t + 41.
Also, note e^(–0.25 u) = e^(–0.25(t+1)) = e^(–0.25) e^(–0.25 t).

Thus the integral now reads

  I = (1/2) e^(–0.25) ∫₀∞ e^(–0.25 t) t^(3/2) (t² – 18t + 41) dt.

Step 2. Expressing the Integral in Terms of Gamma Functions

We can now break the t-integral into three parts:
  I = (1/2) e^(–0.25) [I₁ – 18 I₂ + 41 I₃],
where
  I₁ = ∫₀∞ e^(–0.25 t) t^(3/2+2) dt = ∫₀∞ e^(–0.25 t) t^(7/2) dt,
  I₂ = ∫₀∞ e^(–0.25 t) t^(3/2+1) dt = ∫₀∞ e^(–0.25 t) t^(5/2) dt,
  I₃ = ∫₀∞ e^(–0.25 t) t^(3/2) dt.
Recall the Gamma integral formula:
  ∫₀∞ e^(–λt) t^(ν–1) dt = Γ(ν)/λ^(ν), for Re(ν) > 0.
We have:
• For I₁, we must match t^(7/2) = t^((9/2) – 1) so that ν = 9/2, and λ = 0.25:
  I₁ = Γ(9/2) / (0.25)^(9/2).
• For I₂, t^(5/2) = t^((7/2) – 1) so that ν = 7/2:
  I₂ = Γ(7/2) / (0.25)^(7/2).
• For I₃, t^(3/2) = t^((5/2) – 1) so that ν = 5/2:
  I₃ = Γ(5/2) / (0.25)^(5/2).

Next, recall the Gamma values:
  Γ(9/2) = (7/2)(5/2)(3/2)(1/2) √π = (105/16)√π,
  Γ(7/2) = (5/2)(3/2)(1/2) √π = (15/8)√π,
  Γ(5/2) = (3/2)(1/2) √π = (3/4)√π.

Also note that 0.25 = 1/4, so
  (0.25)^(ν) = (1/4)^(ν) = 4^(–ν).
Thus,
  (0.25)^(9/2) = 4^(–9/2) = 2^(–9),
  (0.25)^(7/2) = 2^(–7),
  (0.25)^(5/2) = 2^(–5).

Substitute these into the expressions for I₁, I₂, and I₃:
  I₁ = (105/16)√π · 2⁹,
  I₂ = (15/8)√π · 2⁷,
  I₃ = (3/4)√π · 2⁵.

Now compute the numerical coefficients:
• 2⁹ = 512, so I₁ = (105/16)√π × 512 = 105 × (512/16) √π = 105 × 32 √π = 3360 √π.
• 2⁷ = 128, so I₂ = (15/8)√π × 128 = 15 × (128/8) √π = 15 × 16 √π = 240 √π.
• 2⁵ = 32, so I₃ = (3/4)√π × 32 = 3 × (32/4) √π = 3 × 8 √π = 24 √π.

Thus, the t-integral becomes

  I = (1/2) e^(–0.25) [3360√π – 18·(240√π) + 41·(24√π)].

Now compute the combination:
  18 × 240 = 4320,
  41 × 24 = 984.
So the bracket is:
  3360√π – 4320√π + 984√π = (3360 – 4320 + 984)√π.
Compute the constant:
  3360 – 4320 = –960, and –960 + 984 = 24.
Thus
  I = (1/2) e^(–0.25) · 24√π = 12 e^(–1/4) √π.

Step 3. Numerical Evaluation

We have
  I = 12 √π e^(–1/4).

Using
  √π ≈ 1.7724538509  and  e^(–0.25) ≈ 0.7788007831,
we compute:
  12 √π ≈ 12 × 1.7724538509 = 21.269446211,
and then
  I ≈ 21.269446211 × 0.7788007831 ≈ 16.5786126590.

Thus the numerical approximation (to 10 decimal places) is 16.5786126590.

Final Answer in JSON Format:
{"answer": "$12\\sqrt{\\pi}e^{-1/4}$", "numerical_answer": "16.5786126590"}