We wish to evaluate

  I = ∫₀² x^(1.0 – 3/2) (2 – x)^(1.0 – 1/2) [1 – 0.5 x (2 – x)]^(–1.0) dx.

Step 1. Rewrite the exponents.
  1.0 – 3/2 = –1/2  and  1.0 – 1/2 = 1/2.
Thus,
  I = ∫₀² x^(–1/2) (2 – x)^(1/2) [1 – 0.5 x (2 – x)]^(–1) dx.

Step 2. Make the substitution u = x – 1.
Let 
  x = u + 1  and  dx = du.
When x = 0, u = –1;  when x = 2, u = 1.
In these new variables the factors become:
  x^(–1/2) = (1 + u)^(–1/2),
  (2 – x)^(1/2) = (1 – u)^(1/2),
and
  1 – 0.5 x (2 – x) = 1 – 0.5 (1 + u)(1 – u) 
           = 1 – 0.5 (1 – u²)
           = 0.5 + 0.5 u² = 0.5 (1 + u²).
Thus the integrand becomes
  (1 + u)^(–1/2)(1 – u)^(1/2) · [0.5 (1 + u²)]^(–1).
Pulling out the constant we have
  [0.5]^(–1) = 2.
Also, the limits are from u = –1 to u = 1. Hence

  I = 2 ∫₋₁¹ (1 – u)^(1/2) (1 + u)^(–1/2) / (1 + u²) du.

Step 3. Make the substitution u = cos θ.
Since u runs from –1 to 1, set
  u = cos θ  so that  du = – sin θ dθ.
When u = –1, cos θ = –1 → θ = π;
when u = 1, cos θ = 1 → θ = 0.
Thus, writing the factors in terms of θ:
  1 – u = 1 – cos θ,
  1 + u = 1 + cos θ.
Recall the half‐angle formulas:
  1 – cos θ = 2 sin²(θ/2),  1 + cos θ = 2 cos²(θ/2),
so that
  (1 – cos θ)^(1/2) = √[2] |sin(θ/2)|  and  (1 + cos θ)^(–1/2) = 1/√[2] |cos(θ/2)|.
For θ in [0, π] the sines and cosines of (θ/2) are nonnegative, so
  (1 – u)^(1/2)(1 + u)^(–1/2) = [√2 sin(θ/2)] [1/(√2 cos(θ/2))] = tan(θ/2).
Also, note that 1 + u² = 1 + cos² θ.
Substituting and also taking care of du = – sinθ dθ (which reverses the integration limits), we find
  I = 2 ∫₍θ=π₎^(θ=0) tan(θ/2)/(1+cos²θ) [– sin θ dθ]
    = 2 ∫₀^(π) tan(θ/2) sinθ/(1+cos²θ) dθ.
Now write tan(θ/2) = sin(θ/2)/cos(θ/2) and note that
  sinθ = 2 sin(θ/2) cos(θ/2).
Thus,
  tan(θ/2) sinθ = [sin(θ/2)/cos(θ/2)] · [2 sin(θ/2) cos(θ/2)] = 2 sin²(θ/2).
So the integral becomes
  I = 2 ∫₀^(π) [2 sin²(θ/2)]/(1+cos²θ) dθ = 4 ∫₀^(π) sin²(θ/2)/(1+cos²θ) dθ.

Step 4. Use a half‐angle identity.
Write sin²(θ/2) in terms of cosine:
  sin²(θ/2) = (1 – cosθ)/2.
Then
  I = 4 ∫₀^(π) (1 – cosθ)/(2[1+cos²θ]) dθ = 2 ∫₀^(π) (1 – cosθ)/(1+cos²θ) dθ.
We now split the integral:
  I = 2 [∫₀^(π) 1/(1+cos²θ)dθ – ∫₀^(π) cosθ/(1+cos²θ)dθ].

Notice that if we let u = sinθ in the second integral, then du = cosθ dθ and the limits (sin0 = 0, sinπ = 0) give an integral that is zero. (More formally, cosθ/(1+cos²θ) is an odd function about θ = π/2, so its integral over [0,π] vanishes.)
Thus,
  I = 2 ∫₀^(π) 1/(1+cos²θ) dθ.

Step 5. Evaluate the remaining integral.
We have
  J = ∫₀^(π) 1/(1+cos²θ)dθ.
Because cos²θ is symmetric about π/2, we may write
  J = 2 ∫₀^(π/2) 1/(1+cos²θ)dθ.
Next, perform the substitution θ → (π/2 – φ). Then cosθ becomes sinφ and the limits remain 0 to π/2. Hence
  J = 2 ∫₀^(π/2) 1/(1+sin²φ)dφ.
A standard integral is known:
  ∫₀^(π/2) dφ/(1+sin²φ) = π/(2√2).
Thus,
  J = 2 · (π/(2√2)) = π/√2.

Returning,
  I = 2J = 2 · (π/√2) = π√2.

Step 6. Numerical approximation.
We have I = π√2. Numerically,
  π √2 ≈ 3.141592653589793 × 1.414213562373095 ≈ 4.442882938158366,
which rounded to 10 decimal places is 4.4428829382.

Thus, the exact answer is π√2 and the numerical value is approximately 4.4428829382.

{"answer": "$\\pi\\sqrt{2}$", "numerical_answer": "4.4428829382"}