<think>
Okay, so I need to compute the definite integral of ln(1 + x + x²) divided by x from 0 to 1. Hmm, let's start by writing down the integral:

∫₀¹ [ln(1 + x + x²)] / x dx

First, I should think about possible methods to tackle this. The integrand has a logarithm divided by x. Maybe integration by parts? Let me consider that. Let u = ln(1 + x + x²) and dv = dx/x. Then du would be the derivative of the logarithm, which is (1 + 2x)/(1 + x + x²) dx, and v would be ln x. Wait, but integration by parts would then lead to uv - ∫ v du. That might complicate things because we'd have ln x multiplied by some rational function. Not sure if that's helpful.

Alternatively, maybe expand the logarithm into a series. Since the logarithm can sometimes be expressed as a power series, which might be easier to integrate term by term. Let's explore that.

First, ln(1 + x + x²). Hmm, note that 1 + x + x² is related to the roots of unity. Specifically, 1 + x + x² = (x³ - 1)/(x - 1) when x ≠ 1. But not sure if that helps here. Alternatively, maybe factor 1 + x + x². The roots are complex, so perhaps not straightforward.

Alternatively, maybe use substitution. Let me think. Let t = x, but not sure. Alternatively, consider expanding the logarithm. Let's recall that ln(1 + y) can be expanded as a power series for |y| < 1. But here, inside the logarithm, we have 1 + x + x². Let me check for x in [0,1], the argument of the logarithm is 1 + x + x². For x between 0 and 1, 1, so 1 + x + x² ranges from 1 to 3. So the argument is always positive, which is good. But the series for ln(1 + y) converges when |y| < 1. Here, 1 + x + x² is 1 + x + x², so if we set y = x + x², then ln(1 + y) where y = x + x². For x in [0,1], y ranges from 0 to 2. So when x is near 1, y = 2, which is outside the radius of convergence (which is 1). Therefore, the series expansion of ln(1 + y) around y=0 would not converge for all x in [0,1]. So that approach might not work directly.

Alternatively, maybe use a substitution to make the logarithm simpler. Let me think. Let’s consider substitution t = x. Wait, not helpful. Maybe substitution u = x² + x + 1. Then du = (2x + 1) dx. But the integrand is ln(u)/x dx. Not sure if that helps.

Alternatively, differentiate under the integral sign. Let’s consider introducing a parameter. Let’s define I(a) = ∫₀¹ [ln(1 + a x + x²)] / x dx. Then compute I'(a) with respect to a. Maybe that could help. Let's try that.

Compute I'(a) = d/da ∫₀¹ [ln(1 + a x + x²)] / x dx = ∫₀¹ [ (x) / (1 + a x + x²) ) ] / x dx = ∫₀¹ 1 / (1 + a x + x²) dx.

So I'(a) = ∫₀¹ 1 / (x² + a x + 1) dx.

This integral can be computed by completing the square in the denominator. Let's do that.

The denominator is x² + a x + 1. Completing the square:

x² + a x + 1 = (x + a/2)^2 + (1 - a²/4)

So the integral becomes ∫₀¹ 1 / [ (x + a/2)^2 + (1 - a²/4) ] dx.

This is a standard integral of the form ∫ 1/(u² + C) du, which is (1/√C) arctan(u / √C) ) + constant.

So let's compute that. Let’s set u = x + a/2, then du = dx. The limits when x=0: u = a/2, and x=1: u = 1 + a/2.

Therefore, I'(a) = ∫_{a/2}^{1 + a/2} 1 / [u² + (1 - a²/4)] du.

The integral is [1 / sqrt(1 - a²/4)] [ arctan( (1 + a/2)/sqrt(1 - a²/4) ) - arctan( (a/2)/sqrt(1 - a²/4) ) ]

But this expression is valid only if 1 - a²/4 > 0, i.e., |a| < 2. Since our original integral is for a=1 (since the original integrand is ln(1 + x + x²)), which is within |a| < 2, so that's okay.

So, simplifying the expression:

Let’s denote C = sqrt(1 - a²/4). Then,

I'(a) = (1/C) [ arctan( (1 + a/2)/C ) - arctan( (a/2)/C ) ]

But this seems a bit complicated. Let me see if we can simplify this expression.

Alternatively, perhaps use substitution. Let’s compute the integral:

∫ 1/(x² + a x + 1) dx from 0 to 1.

The standard integral formula for ∫ dx/(x² + b x + c) is 2/sqrt(4c - b²) arctan( (2x + b)/sqrt(4c - b²) ) ) + constant, when 4c - b² > 0.

In our case, b = a, c = 1. So discriminant is 4*1 - a² = 4 - a². So sqrt(4 - a²). Therefore,

∫ dx/(x² + a x + 1) = 2 / sqrt(4 - a²) [ arctan( (2x + a)/sqrt(4 - a²) ) ] evaluated from 0 to 1.

Therefore,

I'(a) = 2 / sqrt(4 - a²) [ arctan( (2*1 + a)/sqrt(4 - a²) ) - arctan( (2*0 + a)/sqrt(4 - a²) ) ]

Simplify:

= 2 / sqrt(4 - a²) [ arctan( (2 + a)/sqrt(4 - a²) ) - arctan( a / sqrt(4 - a²) ) ]

Hmm, this can be simplified using the identity arctan(u) - arctan(v) = arctan( (u - v)/(1 + uv) ), but I'm not sure if that helps here. Alternatively, perhaps we can relate this to some angle addition.

Alternatively, note that (2 + a)/sqrt(4 - a²) and a / sqrt(4 - a²). Let’s set θ = arctan( a / sqrt(4 - a²) ). Then tan θ = a / sqrt(4 - a²). Let’s square both sides: tan²θ = a² / (4 - a²). Then 1 + tan²θ = 1 + a²/(4 - a²) = 4/(4 - a²). So sec²θ = 4/(4 - a²), so cosθ = sqrt(4 - a²)/2, sinθ = a/2.

Wait, that's interesting. Let’s see:

Let’s set θ = arctan( a / sqrt(4 - a²) ). Then, as above, sinθ = a/2, cosθ = sqrt(4 - a²)/2. Therefore, in a right triangle, opposite side a/2, adjacent sqrt(4 - a²)/2, hypotenuse 1. Wait, hypotenuse would be sqrt( (a/2)^2 + (sqrt(4 - a²)/2)^2 ) = sqrt( a²/4 + (4 - a²)/4 ) = sqrt(4/4) = 1. So yes, θ is an angle that sinθ = a/2, cosθ = sqrt(4 - a²)/2.

Similarly, let’s look at the other term: arctan( (2 + a)/sqrt(4 - a²) ). Let’s denote φ = arctan( (2 + a)/sqrt(4 - a²) ). Then tanφ = (2 + a)/sqrt(4 - a²). Let’s compute sinφ and cosφ.

Let’s set tanφ = (2 + a)/sqrt(4 - a²). Then, in a right triangle, opposite side (2 + a), adjacent sqrt(4 - a²), hypotenuse sqrt( (2 + a)^2 + (4 - a²) ) = sqrt(4 + 4a + a² + 4 - a²) = sqrt(8 + 4a) = 2*sqrt(2 + a).

Therefore, sinφ = (2 + a)/[2 sqrt(2 + a)] ) = sqrt(2 + a)/2, and cosφ = sqrt(4 - a²)/[2 sqrt(2 + a)].

But perhaps there's a relation between θ and φ. Let’s see:

Alternatively, note that φ - θ might be a nice angle. Let’s compute tan(φ - θ) = [tanφ - tanθ] / [1 + tanφ tanθ]

We have tanφ = (2 + a)/sqrt(4 - a²), tanθ = a / sqrt(4 - a²)

So,

tan(φ - θ) = [ (2 + a)/sqrt(4 - a²) - a / sqrt(4 - a²) ] / [1 + ( (2 + a)/sqrt(4 - a²) )( a / sqrt(4 - a²) ) ]

Simplify numerator: [ (2 + a - a) / sqrt(4 - a²) ] = 2 / sqrt(4 - a²)

Denominator: 1 + [ a(2 + a) ] / (4 - a²) = [ (4 - a²) + a(2 + a) ] / (4 - a²) = [4 - a² + 2a + a²] / (4 - a²) = (4 + 2a)/ (4 - a²)

Therefore,

tan(φ - θ) = [2 / sqrt(4 - a²) ] / [ (4 + 2a)/(4 - a²) ) ] = [2 / sqrt(4 - a²) ] * [ (4 - a²)/(4 + 2a) ) ] = [2 (4 - a²) ] / [ sqrt(4 - a²)(4 + 2a) ) ] = [2 sqrt(4 - a²) ] / (4 + 2a) ) = [2 sqrt(4 - a²) ] / [ 2(2 + a) ) ] = sqrt(4 - a²) / (2 + a)

But sqrt(4 - a²) = sqrt( (2 - a)(2 + a) ) = sqrt(2 - a) sqrt(2 + a). Therefore,

tan(φ - θ) = sqrt(2 - a) sqrt(2 + a) / (2 + a) ) = sqrt(2 - a)/sqrt(2 + a) * sqrt(2 + a)/ (2 + a) )? Wait, no:

Wait, sqrt(4 - a²) = sqrt( (2 - a)(2 + a) ), so sqrt(4 - a²)/(2 + a) = sqrt( (2 - a)(2 + a) ) / (2 + a) ) = sqrt( (2 - a)/(2 + a) )

Therefore, tan(φ - θ) = sqrt( (2 - a)/(2 + a) )

Hmm, not sure if that helps. Alternatively, perhaps set t = sqrt( (2 - a)/(2 + a) ), but not sure.

Alternatively, note that sqrt( (2 - a)/(2 + a) ) is tan( something ). Maybe set t = sqrt( (2 - a)/(2 + a) ), then t² = (2 - a)/(2 + a), so cross multiplying: t²(2 + a) = 2 - a => 2 t² + a t² = 2 - a => a(t² + 1) = 2(1 - t²) => a = 2(1 - t²)/(1 + t²). Maybe that substitution could help, but this seems complicated.

Alternatively, perhaps we can express I'(a) in terms of φ - θ. Since I'(a) = 2 / sqrt(4 - a²) [ φ - θ ].

But φ - θ = arctan( (2 + a)/sqrt(4 - a²) ) - arctan( a / sqrt(4 - a²) )

But from the previous calculation, tan(φ - θ) = sqrt( (2 - a)/(2 + a) )

Therefore, φ - θ = arctan( sqrt( (2 - a)/(2 + a) ) )

But sqrt( (2 - a)/(2 + a) ) can be written as tan( (π/4 - a/4) ) or something? Not sure.

Alternatively, let’s set t = sqrt( (2 - a)/(2 + a) ). Then t = sqrt( (2 - a)/(2 + a) ). Let’s square both sides: t² = (2 - a)/(2 + a). Then, solving for a:

t²(2 + a) = 2 - a => 2 t² + a t² = 2 - a => a(t² + 1) = 2(1 - t²) => a = 2(1 - t²)/(1 + t²)

But this substitution might not lead us anywhere. Alternatively, perhaps we can relate this to trigonometric substitution. Let’s consider a = 2 cos θ. Then, since |a| < 2, θ would be real. Let’s try that.

Let’s set a = 2 cos θ, where θ ∈ (0, π). Then sqrt(4 - a²) = sqrt(4 - 4 cos²θ) = 2 sinθ.

Then, tan(φ - θ) = sqrt( (2 - a)/(2 + a) ) = sqrt( (2 - 2 cosθ)/(2 + 2 cosθ) ) = sqrt( (1 - cosθ)/(1 + cosθ) ) = tan(θ/2). Because (1 - cosθ)/(1 + cosθ) = tan²(θ/2). Therefore, sqrt( (1 - cosθ)/(1 + cosθ) ) = |tan(θ/2)|. Since θ is between 0 and π, tan(θ/2) is positive, so it's equal to tan(θ/2). Therefore, tan(φ - θ) = tan(θ/2). Therefore, φ - θ = θ/2 + kπ. But since θ is between 0 and π, and φ and θ are arctans which are between 0 and π/2 (since the arguments are positive), then φ - θ = θ/2. Therefore, φ = (3θ)/2.

But φ = arctan( (2 + a)/sqrt(4 - a²) ) = arctan( (2 + 2 cosθ)/ (2 sinθ) ) = arctan( (1 + cosθ)/ sinθ ) = arctan( cot(θ/2) ) = arctan( tan( (π/2 - θ/2) ) ) = π/2 - θ/2.

Wait, but earlier we had φ = 3θ/2. Wait, this seems conflicting. Let me check.

Wait, if a = 2 cosθ, then:

φ = arctan( (2 + a)/sqrt(4 - a²) ) = arctan( (2 + 2 cosθ)/ (2 sinθ) ) = arctan( (1 + cosθ)/ sinθ )

Using the identity (1 + cosθ)/sinθ = cot(θ/2). Therefore, arctan(cot(θ/2)) = arctan(tan(π/2 - θ/2)) = π/2 - θ/2.

Similarly, θ was defined as a = 2 cosθ, so θ = arccos(a/2). Therefore, φ = π/2 - θ/2 = π/2 - (1/2) arccos(a/2).

Similarly, θ = arccos(a/2). So, φ - θ = π/2 - (1/2) arccos(a/2) - arccos(a/2) = π/2 - (3/2) arccos(a/2). But earlier we had φ - θ = θ/2. Hmm, this seems inconsistent. Maybe my substitution is not correct.

Alternatively, perhaps I made a mistake in the substitution steps. Let me re-examine.

If a = 2 cosθ, then sqrt(4 - a²) = 2 sinθ. Then:

I'(a) = 2 / (2 sinθ) [ φ - θ ] where φ = π/2 - θ/2, and θ = arccos(a/2). Wait, but θ is arccos(a/2), so θ is in (0, π). Then:

φ - θ = π/2 - θ/2 - θ = π/2 - (3θ)/2.

But then I'(a) = (1/sinθ) [ π/2 - (3θ)/2 ].

But θ = arccos(a/2), so sinθ = sqrt(1 - (a²/4)).

Therefore, I'(a) = [ π/2 - (3/2) arccos(a/2) ] / sqrt(1 - a²/4 )

But this seems complicated. Maybe there's a better way.

Alternatively, perhaps integrating I'(a) from a=0 to a=1. Since the original integral is I(1), and we need to compute I(1). But we have I'(a) expressed in terms of arctans. Let’s recall that I(a) is the integral from 0 to1 of [ln(1 + a x + x²)] / x dx. When a=0, the integrand becomes [ln(1 + x²)] / x dx. Wait, but when a=0, 1 + 0 + x² = 1 + x². So I(0) = ∫₀¹ ln(1 + x²)/x dx. Hmm, but maybe we can compute I(0) separately.

Alternatively, since we need I(1), and we have I'(a) from a=0 to a=1. So I(1) = I(0) + ∫₀¹ I'(a) da.

But if we can compute I(0) and then compute the integral of I'(a) from 0 to1, then we can get the desired result.

But first, let's compute I(0):

I(0) = ∫₀¹ [ln(1 + x²)] / x dx.

Let’s make substitution t = x², so dt = 2x dx, so dx = dt/(2 sqrt(t)). Then,

I(0) = ∫₀¹ [ln(1 + t)] / sqrt(t) * (dt/(2 sqrt(t))) ) = (1/2) ∫₀¹ ln(1 + t) / t dt.

But ∫ ln(1 + t)/t dt is a standard integral known as the dilogarithm function. Specifically, ∫₀¹ ln(1 + t)/t dt = -Li₂(-t) evaluated from 0 to1, which is -Li₂(-1) + Li₂(0). Since Li₂(0) = 0, and Li₂(-1) = -π²/12. Therefore, -Li₂(-1) = π²/12. Therefore, I(0) = (1/2)(π²/12) = π²/24.

Alternatively, we can compute ∫₀¹ ln(1 + t)/t dt by expanding ln(1 + t) as a power series. For |t| <1, ln(1 + t) = Σ_{n=1}^∞ (-1)^{n+1} t^n /n. But integrating from 0 to1, even though t=1 is at the boundary, the series converges conditionally there. So,

∫₀¹ ln(1 + t)/t dt = Σ_{n=1}^∞ (-1)^{n+1} ∫₀¹ t^{n-1} /n dt = Σ_{n=1}^∞ (-1)^{n+1} [ t^n /n² ] from 0 to1 = Σ_{n=1}^∞ (-1)^{n+1} /n².

This is the Dirichlet eta function at 2: η(2) = (1 - 2^{1 - 2}) ζ(2) = (1 - 1/2) π²/6 = π²/12. Therefore, the integral is π²/12, so I(0) = (1/2)(π²/12) = π²/24.

Okay, so I(0) = π²/24.

Now, we need to compute I(1) = I(0) + ∫₀¹ I'(a) da.

So, I(1) = π²/24 + ∫₀¹ [2 / sqrt(4 - a²) ( arctan( (2 + a)/sqrt(4 - a²) ) - arctan( a / sqrt(4 - a²) ) ) ] da.

This integral looks complicated. Let’s see if we can find a substitution to simplify it.

Let’s denote the expression inside the integral as:

2 / sqrt(4 - a²) [ arctan( (2 + a)/sqrt(4 - a²) ) - arctan( a / sqrt(4 - a²) ) ] da.

Let’s consider substitution u = 2 sinθ, but not sure. Alternatively, let’s use the substitution we tried earlier, a = 2 cosθ. Let’s try that.

Let’s set a = 2 cosθ, so da = -2 sinθ dθ. When a=0, θ=π/2; when a=1, θ=arccos(1/2)=π/3.

Then, sqrt(4 - a²) = sqrt(4 - 4 cos²θ) = 2 sinθ.

The expression inside the integral becomes:

2 / (2 sinθ) [ arctan( (2 + 2 cosθ)/ (2 sinθ) ) - arctan( 2 cosθ / (2 sinθ) ) ] * (-2 sinθ dθ )

Simplify:

= [1/sinθ] [ arctan( (1 + cosθ)/sinθ ) - arctan( cotθ ) ] * (-2 sinθ dθ )

= [1/sinθ] [ arctan( cot(θ/2) ) - arctan( cotθ ) ] * (-2 sinθ dθ )

Note that (1 + cosθ)/sinθ = cot(θ/2). Because:

(1 + cosθ)/sinθ = 2 cos²(θ/2) / (2 sin(θ/2) cos(θ/2)) ) = cot(θ/2).

Similarly, cotθ = cosθ/sinθ.

Therefore, arctan(cot(θ/2)) = arctan(tan(π/2 - θ/2)) = π/2 - θ/2, since θ is between π/3 and π/2, so π/2 - θ/2 is between π/2 - π/4 = π/4 and π/2 - π/6 = π/3, which is within the principal value of arctan.

Similarly, arctan(cotθ) = arctan(tan(π/2 - θ)) = π/2 - θ, again since θ is between π/3 and π/2, so π/2 - θ is between 0 and π/6.

Therefore, the expression becomes:

[1/sinθ] [ (π/2 - θ/2) - (π/2 - θ) ] * (-2 sinθ dθ )

Simplify inside the brackets:

(π/2 - θ/2 - π/2 + θ) = (θ/2)

Therefore, the entire integral becomes:

[1/sinθ] * (θ/2) * (-2 sinθ dθ ) = [θ/2 * (-2) dθ ] = -θ dθ

Therefore, the integral ∫₀¹ I'(a) da becomes ∫_{π/2}^{π/3} -θ dθ = ∫_{π/3}^{π/2} θ dθ = [ (θ²)/2 ]_{π/3}^{π/2} = ( (π/2)² /2 ) - ( (π/3)² /2 ) = ( π²/8 - π²/18 ) / 1 = ( (9π² - 4π²)/72 ) = 5π²/72.

Therefore, the integral ∫₀¹ I'(a) da = 5π²/72.

Therefore, I(1) = I(0) + 5π²/72 = π²/24 + 5π²/72 = (3π² + 5π²)/72 = 8π²/72 = π²/9.

Wait, that's nice! So the integral evaluates to π²/9.

But let me verify this calculation again to make sure.

First, substitution a = 2 cosθ, da = -2 sinθ dθ. When a=0, θ=π/2; a=1, θ=π/3.

Then, the integral becomes:

∫_{π/2}^{π/3} [ -θ dθ ] = ∫_{π/3}^{π/2} θ dθ = [θ²/2]_{π/3}^{π/2} = ( (π/2)^2 /2 ) - ( (π/3)^2 /2 ) = (π²/8) - (π²/18) = (9π² - 4π²)/72 = 5π²/72.

Then, I(1) = π²/24 + 5π²/72 = (3π² + 5π²)/72 = 8π²/72 = π²/9.

Yes, that seems correct. Therefore, the exact value of the integral is π²/9.

Now, to compute the numerical approximation. π²/9 is approximately (9.8696044)/9 ≈ 1.096622711 approximately. Let me compute this more accurately.

π ≈ 3.141592653589793

π² ≈ 9.869604401089358

Divided by 9: 9.869604401089358 / 9 ≈ 1.0966227112321508

Rounded to 10 decimal places: 1.0966227112

But let me verify using numerical integration to check.

Alternatively, compute the integral numerically. Let's approximate ∫₀¹ ln(1 + x + x²)/x dx.

We can use a calculator or approximate using series expansion.

Alternatively, since we know the exact answer is π²/9 ≈ 1.0966227112321508, so rounded to 10 decimal places is 1.0966227112.

But to confirm, let's compute it numerically.

Alternatively, use substitution. Let’s expand ln(1 + x + x²) as a power series and integrate term by term.

Note that 1 + x + x² = (x³ - 1)/(x - 1) for x ≠1. But perhaps we can use generating functions.

Alternatively, note that ln(1 + x + x²) = ln( (x³ - 1)/(x - 1) ) = ln(1 - x³) - ln(1 - x). But for x in (0,1), this is valid.

Therefore, ln(1 + x + x²) = ln(1 - x³) - ln(1 - x).

Therefore, the integral becomes ∫₀¹ [ln(1 - x³) - ln(1 - x)] / x dx = ∫₀¹ ln(1 - x³)/x dx - ∫₀¹ ln(1 - x)/x dx.

We know that ∫₀¹ ln(1 - x)/x dx = -π²/6 (since it's the dilogarithm Li₂(1) = π²/6, but with a negative sign).

Similarly, ∫₀¹ ln(1 - x³)/x dx. Let’s make substitution t = x³, so x = t^{1/3}, dx = (1/3) t^{-2/3} dt. Then,

∫₀¹ ln(1 - x³)/x dx = ∫₀¹ ln(1 - t)/t^{1/3} * (1/3) t^{-2/3} dt = (1/3) ∫₀¹ ln(1 - t) t^{-1} dt = (1/3) ∫₀¹ ln(1 - t)/t dt = (1/3)( -π²/6 ) = -π²/18.

Therefore, the original integral is:

-π²/18 - (-π²/6) = -π²/18 + π²/6 = ( -π² + 3π² ) / 18 = 2π²/18 = π²/9.

Which confirms the previous result. Therefore, the exact value is π²/9 ≈ 1.0966227112321508.

Rounded to 10 decimal places, that's 1.0966227112.

So the final answer is π²/9 with numerical approximation 1.0966227112.
</think>

{"answer": "\\frac{\\pi^2}{9}", "numerical_answer": "1.0966227112"}