
To solve the definite integral \(\int\limits_0^2 x H_{3}\left(\sqrt{x(2-x)}\right)dx\), we follow these steps:

### Step 1: Simplify the Integrand Using Substitution
First, recall the 3rd Hermite polynomial: \(H_3(z) = 8z^3 - 12z\). The integrand becomes:
\[
x \cdot H_3\left(\sqrt{x(2-x)}\right) = x \left[8\left(\sqrt{x(2-x)}\right)^3 - 12\sqrt{x(2-x)}\right].
\]

### Step 2: Substitute \(x = 1 + u\)
To simplify the expression under the square root, use the substitution \(x = 1 + u\), so \(dx = du\). When \(x = 0\), \(u = -1\); when \(x = 2\), \(u = 1\). The term \(x(2-x)\) becomes:
\[
(1 + u)(1 - u) = 1 - u^2,
\]
so \(\sqrt{x(2-x)} = \sqrt{1 - u^2}\). The integral transforms to:
\[
\int_{-1}^1 (1 + u) H_3\left(\sqrt{1 - u^2}\right) du.
\]

### Step 3: Split the Integral
Split the integral into two parts:
\[
\int_{-1}^1 (1 + u) H_3\left(\sqrt{1 - u^2}\right) du = \int_{-1}^1 H_3\left(\sqrt{1 - u^2}\right) du + \int_{-1}^1 u H_3\left(\sqrt{1 - u^2}\right) du.
\]
The second integral involves an odd function (since \(u\) is odd and \(H_3\left(\sqrt{1 - u^2}\right)\) is even), so it vanishes over the symmetric interval \([-1, 1]\). Thus, the integral reduces to:
\[
\int_{-1}^1 H_3\left(\sqrt{1 - u^2}\right) du.
\]

### Step 4: Expand \(H_3\left(\sqrt{1 - u^2}\right)\)
Using \(H_3(z) = 8z^3 - 12z\), we substitute \(z = \sqrt{1 - u^2}\):
\[
H_3\left(\sqrt{1 - u^2}\right) = 8(1 - u^2)^{3/2} - 12(1 - u^2)^{1/2}.
\]

### Step 5: Evaluate the Integral
The integral becomes:
\[
\int_{-1}^1 \left[8(1 - u^2)^{3/2} - 12(1 - u^2)^{1/2}\right] du.
\]
Using symmetry and standard integrals for \((1 - u^2)^n\) over \([-1, 1]\):
- \(\int_{-1}^1 (1 - u^2)^{3/2} du = \frac{3\pi}{8}\)
- \(\int_{-1}^1 (1 - u^2)^{1/2} du = \frac{\pi}{2}\)

Thus:
\[
8 \cdot \frac{3\pi}{8} - 12 \cdot \frac{\pi}{2} = 3\pi - 6\pi = -3\pi.
\]

### Numerical Approximation
The numerical value of \(-3\pi\) is approximately \(-9.4247779608\) (rounded to 10 decimal places).

{"answer": "$-3\\pi$", "numerical_answer": "-9.4247779608"}