Let's denote the integral as \( I \):

\[
I = \int_0^1 x \arcsin x \arccos x\,dx
\]

Let's proceed step by step.

---

### **Step 1: Recognize \(\arcsin x \arccos x\) reduction**

Recall that:
\[
\arcsin x + \arccos x = \frac{\pi}{2} \implies \arccos x = \frac{\pi}{2} - \arcsin x
\]

Hence:
\[
\arcsin x \arccos x = \arcsin x \left( \frac{\pi}{2} - \arcsin x \right ) = \frac{\pi}{2} \arcsin x - (\arcsin x)^2
\]

So:
\[
I = \int_0^1 x \arcsin x \arccos x\,dx = \frac{\pi}{2} \int_0^1 x \arcsin x\,dx - \int_0^1 x (\arcsin x)^2 dx
\]

Let:
\[
I_1 = \int_0^1 x \arcsin x\,dx
\]
\[
I_2 = \int_0^1 x (\arcsin x)^2 dx
\]

So:
\[
I = \frac{\pi}{2} I_1 - I_2
\]

---

### **Step 2: Calculate \(I_1 = \int_0^1 x \arcsin x\,dx\)**

Let’s use integration by parts:
Let \( u = \arcsin x \implies du = \frac{dx}{\sqrt{1-x^2}} \)
Let \( dv = x dx \implies v = \frac{1}{2} x^2 \)

So:
\[
\int x \arcsin x\,dx = \frac{1}{2} x^2 \arcsin x - \frac{1}{2} \int \frac{x^2}{\sqrt{1-x^2}} dx
\]

Now, at the bounds \(x=0\) and \(x=1\):

First, plug in 0:
\[
x^2 \arcsin x \Big|_{x=0} = 0
\]
Plug in 1:
\[
x^2 \arcsin x \Big|_{x=1} = 1 \cdot \arcsin 1 = \frac{\pi}{2}
\]
So:
\[
\int_0^1 x \arcsin x\,dx = \frac{1}{2}\left[ \frac{\pi}{2} - 0 \right]
- \frac{1}{2} \int_0^1 \frac{x^2}{\sqrt{1-x^2}} dx
\]
\[
= \frac{\pi}{4} - \frac{1}{2} \int_0^1 \frac{x^2}{\sqrt{1-x^2}} dx
\]

Let’s compute \(J = \int_0^1 \frac{x^2}{\sqrt{1-x^2}} dx\):

Let \( x = \sin \theta, dx = \cos\theta d\theta \), as \( x \) goes from 0 to 1, \( \theta \) goes from 0 to \(\frac{\pi}{2}\):

\[
x^2 = \sin^2\theta,\ \sqrt{1-x^2} = \cos\theta
\]

So:
\[
J = \int_{\theta=0}^{\pi/2} \frac{\sin^2 \theta}{\cos\theta} \cos\theta d\theta = \int_0^{\pi/2} \sin^2\theta d\theta
\]

We know:
\[
\int \sin^2\theta d\theta = \frac{\theta}{2} - \frac{1}{4}\sin 2\theta
\]

Evaluate from 0 to \(\frac{\pi}{2}\):

\[
\frac{\pi}{4} - \frac{1}{4} \sin(\pi) - \left( 0 - \frac{1}{4}\sin 0 \right ) = \frac{\pi}{4}
\]

So,
\[
J = \frac{\pi}{4}
\]

Therefore,
\[
I_1 = \frac{\pi}{4} - \frac{1}{2} \cdot \frac{\pi}{4} = \frac{\pi}{4} - \frac{\pi}{8} = \frac{\pi}{8}
\]

---

### **Step 3: Calculate \(I_2 = \int_0^1 x (\arcsin x)^2 dx\)**

Let’s use integration by parts:

Let \( u = (\arcsin x)^2,\ du = 2 \arcsin x \frac{1}{\sqrt{1-x^2}} dx \)
Let \( dv = x dx,\ v = \frac{1}{2}x^2 \)

So:
\[
I_2 = \int_0^1 x (\arcsin x)^2 dx = \frac{1}{2} x^2 (\arcsin x)^2 \Big|_0^1 - \frac{1}{2}\int_0^1 x^2 \cdot 2 \arcsin x \frac{1}{\sqrt{1-x^2}} dx
\]
\[
= \frac{1}{2} x^2 (\arcsin x)^2 \Big|_0^1 - \int_0^1 x^2 \arcsin x \frac{1}{\sqrt{1-x^2}} dx
\]

Compute the first term at bounds:

For \(x=0\), \(x^2(\arcsin x)^2 = 0\)

For \(x=1\), \(1 \cdot (\arcsin 1)^2 = (\frac{\pi}{2})^2 = \frac{\pi^2}{4}\)

So,
\[
\frac{1}{2} x^2 (\arcsin x)^2 \Big|_0^1 = \frac{\pi^2}{8}
\]

Let’s denote
\[
K = \int_0^1 x^2 \arcsin x \frac{1}{\sqrt{1-x^2}} dx
\]
So,
\[
I_2 = \frac{\pi^2}{8} - K
\]

Now, let’s compute \(K\):

Let \( x = \sin\theta \) as before, \( x^2 = \sin^2\theta \), \( \arcsin x = \theta \), \( \sqrt{1-x^2} = \cos\theta \), \( dx = \cos\theta d\theta \). As \( x \) goes from 0 to 1, \( \theta \) goes from 0 to \(\frac{\pi}{2}\):

So,
\[
K = \int_0^1 x^2 \arcsin x \frac{1}{\sqrt{1-x^2}} dx = \int_{\theta=0}^{\pi/2} \sin^2\theta \theta \cdot \frac{1}{\cos\theta}\cdot \cos\theta d\theta = \int_0^{\pi/2} \theta \sin^2\theta d\theta
\]

So,
\[
K = \int_0^{\pi/2} \theta \sin^2\theta d\theta
\]

Let’s compute \( K \):

\[
\sin^2\theta = \frac{1 - \cos 2\theta}{2}
\]
So:
\[
K = \int_0^{\pi/2} \theta \frac{1 - \cos2\theta}{2} d\theta = \frac{1}{2}\int_0^{\pi/2} \theta d\theta - \frac{1}{2}\int_0^{\pi/2} \theta \cos 2\theta d\theta
\]

Compute both terms:

**First term:**
\[
\int_0^{\pi/2} \theta d\theta = \left[ \frac{1}{2} \theta^2 \right]_0^{\pi/2} = \frac{1}{2} \left( \frac{\pi}{2} \right)^2 = \frac{\pi^2}{8}
\]

**Second term: \( \int_0^{\pi/2} \theta \cos 2\theta\,d\theta \) via integration by parts:**

Let \( u = \theta, dv = \cos 2\theta d\theta \implies v = \frac{1}{2}\sin 2\theta \)
So:
\[
\int \theta \cos 2\theta d\theta = \theta \cdot \frac{1}{2}\sin 2\theta - \int \frac{1}{2}\sin 2\theta d\theta
= \frac{1}{2}\theta \sin 2\theta + \frac{1}{4}\cos 2\theta + C
\]

Evaluate from 0 to \(\frac{\pi}{2}\):

At \(\theta = \frac{\pi}{2}\):

- \(\sin 2\theta = \sin \pi = 0\)
- \(\cos 2\theta = \cos \pi = -1\)

at \(\theta=0\), both terms are 0 and 1:

So,
\[
\frac{1}{2}\cdot \frac{\pi}{2} \cdot 0 + \frac{1}{4}(-1) - \left(0 + \frac{1}{4}(1)\right) = 0 - \frac{1}{4} - 0 - \frac{1}{4} = -\frac{1}{2}
\]

Thus,
\[
\int_0^{\pi/2} \theta \cos 2\theta d\theta = -\frac{1}{2}
\]

So,
\[
K = \frac{1}{2}\cdot\frac{\pi^2}{8} - \frac{1}{2}(-\frac{1}{2}) = \frac{\pi^2}{16} + \frac{1}{4}
\]

---

### **Step 4: Assemble everything**

Recall:
\[
I_1 = \frac{\pi}{8}
\]
\[
I_2 = \frac{\pi^2}{8} - \left( \frac{\pi^2}{16} + \frac{1}{4} \right ) = \frac{2\pi^2}{16} - \frac{\pi^2}{16} - \frac{1}{4}
= \frac{\pi^2}{16} - \frac{1}{4}
\]

Plug into original formula:
\[
I = \frac{\pi}{2} I_1 - I_2 = \frac{\pi}{2} \cdot \frac{\pi}{8} - \left( \frac{\pi^2}{16} - \frac{1}{4} \right )
= \frac{\pi^2}{16} - \frac{\pi^2}{16} + \frac{1}{4}
= \frac{1}{4}
\]

---

## **Step 5: Final answers**

### **Exact answer:**
\[
I = \frac{1}{4}
\]

### **Numerical approximation:**
\[
I \approx 0.25
\]

---

```json
{"answer": "\\frac{1}{4}", "numerical_answer": "0.25"}
```