


To solve the definite integral \(\int\limits_0^2 x^{-1/2} H_{3}\left(\sqrt[4]{x(2-x)}\right) dx\), we follow these steps:

### Step 1: Expand the Hermite Polynomial
The 3rd Hermite polynomial is \(H_3(z) = 8z^3 - 12z\). Substituting \(z = \sqrt[4]{x(2-x)}\), the integrand becomes:
\[
x^{-1/2} \left(8\left(\sqrt[4]{x(2-x)}\right)^3 - 12\sqrt[4]{x(2-x)}\right)
\]
Simplifying \(z^3 = \left(x(2-x)\right)^{3/4}\) and \(z = \left(x(2-x)\right)^{1/4}\), the integrand splits into two terms:
\[
8x^{-1/2} \left(x(2-x)\right)^{3/4} - 12x^{-1/2} \left(x(2-x)\right)^{1/4}
\]

### Step 2: Simplify the Integrand
For the first term:
\[
x^{-1/2} \left(x(2-x)\right)^{3/4} = x^{-1/2} \cdot x^{3/4}(2-x)^{3/4} = x^{1/4}(2-x)^{3/4}
\]
For the second term:
\[
x^{-1/2} \left(x(2-x)\right)^{1/4} = x^{-1/2} \cdot x^{1/4}(2-x)^{1/4} = x^{-1/4}(2-x)^{1/4}
\]
Thus, the integral becomes:
\[
8 \int_0^2 x^{1/4}(2-x)^{3/4} dx - 12 \int_0^2 x^{-1/4}(2-x)^{1/4} dx
\]

### Step 3: Evaluate the Integrals Using Beta Functions
Both integrals are of the form \(\int_0^a t^{p-1}(a-t)^{q-1} dt\), which relates to the Beta function \(B(p, q) = \int_0^1 t^{p-1}(1-t)^{q-1} dt\) via substitution \(t = au\).

#### First Integral: \(I_1 = \int_0^2 x^{1/4}(2-x)^{3/4} dx\)
Let \(x = 2u\), so \(dx = 2du\). Then:
\[
I_1 = 2 \int_0^1 (2u)^{1/4}(2-2u)^{3/4} du = 2 \cdot 2^{1/4 + 3/4} \int_0^1 u^{1/4}(1-u)^{3/4} du = 4 \int_0^1 u^{5/4 - 1}(1-u)^{7/4 - 1} du = 4 B\left(\frac{5}{4}, \frac{7}{4}\right)
\]
Using \(B(p, q) = \frac{\Gamma(p)\Gamma(q)}{\Gamma(p+q)}\) and \(\Gamma(3) = 2\):
\[
I_1 = 4 \cdot \frac{\Gamma\left(\frac{5}{4}\right)\Gamma\left(\frac{7}{4}\right)}{\Gamma(3)} = 2 \Gamma\left(\frac{5}{4}\right)\Gamma\left(\frac{7}{4}\right)
\]

#### Second Integral: \(I_2 = \int_0^2 x^{-1/4}(2-x)^{1/4} dx\)
Similarly, let \(x = 2u\):
\[
I_2 = 2 \int_0^1 (2u)^{-1/4}(2-2u)^{1/4} du = 2 \cdot 2^{-1/4 + 1/4} \int_0^1 u^{-1/4}(1-u)^{1/4} du = 2 \int_0^1 u^{3/4 - 1}(1-u)^{5/4 - 1} du = 2 B\left(\frac{3}{4}, \frac{5}{4}\right)
\]
Using \(\Gamma(2) = 1\):
\[
I_2 = 2 \cdot \frac{\Gamma\left(\frac{3}{4}\right)\Gamma\left(\frac{5}{4}\right)}{\Gamma(2)} = 2 \Gamma\left(\frac{3}{4}\right)\Gamma\left(\frac{5}{4}\right)
\]

### Step 4: Simplify Using Gamma Function Properties
Using \(\Gamma(z+1) = z\Gamma(z)\) and the reflection formula \(\Gamma(z)\Gamma(1-z) = \frac{\pi}{\sin(\pi z)}\):
- \(\Gamma\left(\frac{5}{4}\right) = \frac{1}{4}\Gamma\left(\frac{1}{4}\right)\)
- \(\Gamma\left(\frac{7}{4}\right) = \frac{3}{4}\Gamma\left(\frac{3}{4}\right)\)
- \(\Gamma\left(\frac{1}{4}\right)\Gamma\left(\frac{3}{4}\right) = \frac{\pi}{\sin\left(\frac{\pi}{4}\right)} = \pi\sqrt{2}\)

Substituting these into \(I_1\) and \(I_2\):
\[
I_1 = 2 \cdot \frac{1}{4}\Gamma\left(\frac{1}{4}\right) \cdot \frac{3}{4}\Gamma\left(\frac{3}{4}\right) = \frac{3}{8} \pi\sqrt{2}
\]
\[
I_2 = 2 \cdot \Gamma\left(\frac{3}{4}\right) \cdot \frac{1}{4}\Gamma\left(\frac{1}{4}\right) = \frac{1}{2} \pi\sqrt{2}
\]

### Step 5: Combine Results
The original integral is:
\[
8I_1 - 12I_2 = 8 \cdot \frac{3}{8}\pi\sqrt{2} - 12 \cdot \frac{1}{2}\pi\sqrt{2} = 3\pi\sqrt{2} - 6\pi\sqrt{2} = -3\pi\sqrt{2}
\]

### Numerical Approximation
Using \(\pi \approx 3.141592653589793\) and \(\sqrt{2} \approx 1.4142135623730951\):
\[
-3\pi\sqrt{2} \approx -3 \cdot 3.141592653589793 \cdot 1.4142135623730951 \approx -13.3286487257
\]

{"answer": "$-3\\pi\\sqrt{2}$", "numerical_answer": "-13.3286487257"}