To solve the definite integral 

\[
\int\limits_0^1 x^{-1} \ln x \ln \left( \frac{2 + x}{2 - x} \right) \, dx,
\]

we proceed with the following steps:

### Step 1: Simplify the Integrand
First, observe that the integrand can be rewritten using the properties of logarithms:

\[
\ln \left( \frac{2 + x}{2 - x} \right) = \ln(2 + x) - \ln(2 - x).
\]

Thus, the integral becomes:

\[
\int\limits_0^1 \frac{\ln x}{x} \left( \ln(2 + x) - \ln(2 - x) \right) \, dx = \int\limits_0^1 \frac{\ln x \ln(2 + x)}{x} \, dx - \int\limits_0^1 \frac{\ln x \ln(2 - x)}{x} \, dx.
\]

### Step 2: Introduce a Parameter and Differentiate
Consider the following parameterized integrals:

\[
I(a) = \int\limits_0^1 \frac{\ln x \ln(1 + a x)}{x} \, dx,
\]
\[
J(a) = \int\limits_0^1 \frac{\ln x \ln(1 - a x)}{x} \, dx.
\]

We can express our original integral in terms of \( I(a) \) and \( J(a) \):

\[
\int\limits_0^1 \frac{\ln x \ln(2 + x)}{x} \, dx = \ln 2 \int\limits_0^1 \frac{\ln x}{x} \, dx + I\left(\frac{1}{2}\right),
\]
\[
\int\limits_0^1 \frac{\ln x \ln(2 - x)}{x} \, dx = \ln 2 \int\limits_0^1 \frac{\ln x}{x} \, dx + J\left(\frac{1}{2}\right).
\]

However, the integral \( \int_0^1 \frac{\ln x}{x} \, dx \) diverges, which suggests that we need a different approach.

### Step 3: Alternative Approach Using Series Expansion
Expand the logarithm functions into their Taylor series around \( x = 0 \):

\[
\ln(2 + x) = \ln 2 + \sum_{n=1}^\infty \frac{(-1)^{n+1} x^n}{n 2^n},
\]
\[
\ln(2 - x) = \ln 2 - \sum_{n=1}^\infty \frac{x^n}{n 2^n}.
\]

Substituting these into the integral:

\[
\int\limits_0^1 \frac{\ln x}{x} \left( \ln(2 + x) - \ln(2 - x) \right) \, dx = \int\limits_0^1 \frac{\ln x}{x} \left( \sum_{n=1}^\infty \frac{(-1)^{n+1} x^n}{n 2^n} + \sum_{n=1}^\infty \frac{x^n}{n 2^n} \right) \, dx.
\]

Combine the series:

\[
\sum_{n=1}^\infty \left( \frac{(-1)^{n+1}}{n 2^n} + \frac{1}{n 2^n} \right) x^n = \sum_{n=1}^\infty \frac{1 + (-1)^{n+1}}{n 2^n} x^n.
\]

Notice that \( 1 + (-1)^{n+1} \) is 2 for odd \( n \) and 0 for even \( n \). Thus, the series simplifies to:

\[
\sum_{k=0}^\infty \frac{2}{(2k + 1) 2^{2k + 1}} x^{2k + 1} = \sum_{k=0}^\infty \frac{x^{2k + 1}}{(2k + 1) 2^{2k}}.
\]

Now, the integral becomes:

\[
\int\limits_0^1 \frac{\ln x}{x} \sum_{k=0}^\infty \frac{x^{2k + 1}}{(2k + 1) 2^{2k}} \, dx = \sum_{k=0}^\infty \frac{1}{(2k + 1) 2^{2k}} \int\limits_0^1 x^{2k} \ln x \, dx.
\]

### Step 4: Evaluate the Inner Integral
The inner integral is:

\[
\int\limits_0^1 x^{2k} \ln x \, dx = -\frac{1}{(2k + 1)^2}.
\]

This can be derived by integration by parts or by recognizing it as a standard result.

### Step 5: Sum the Series
Substituting the inner integral back:

\[
\sum_{k=0}^\infty \frac{1}{(2k + 1) 2^{2k}} \left( -\frac{1}{(2k + 1)^2} \right) = -\sum_{k=0}^\infty \frac{1}{(2k + 1)^3 2^{2k}}.
\]

This series can be expressed in terms of the polylogarithm function \( \text{Li}_3 \):

\[
-\sum_{k=0}^\infty \frac{1}{(2k + 1)^3 2^{2k}} = -\text{Li}_3\left(\frac{1}{2}\right) + \frac{1}{8} \text{Li}_3(1).
\]

However, a more straightforward evaluation is possible by recognizing the series:

\[
\sum_{k=0}^\infty \frac{1}{(2k + 1)^3 2^{2k}} = \frac{7 \zeta(3)}{8}.
\]

Thus, the integral evaluates to:

\[
-\frac{7 \zeta(3)}{8}.
\]

### Step 6: Numerical Approximation
The numerical value of \( \zeta(3) \) (Ap√©ry's constant) is approximately 1.2020569032. Therefore:

\[
-\frac{7 \times 1.2020569032}{8} \approx -1.0517997903.
\]

### Final Answer
The exact answer is \( -\frac{7}{8} \zeta(3) \), and its numerical approximation is approximately -1.0517997903.

```json
{"answer": "-\\frac{7}{8} \\zeta(3)", "numerical_answer": "-1.0517997903"}
```