Let's work through the definite integral:
\[
I = \int_0^{2} x^{1/2} (2-x)^{1/2} \cos\left( \sqrt{x(2-x)} \right) dx
\]

## Step 1: Substitution to Simplify

Let’s try the substitution:
\[
x = 2\sin^2\theta \implies dx = 4\sin\theta\cos\theta\, d\theta = 2\sin(2\theta)d\theta
\]
When \( x = 0 \), \(\theta = 0\); when \( x = 2 \), \(\sin^2\theta = 1\), so \(\theta = \frac{\pi}{2}\).

Also,
\[
2-x = 2 - 2\sin^2\theta = 2\cos^2\theta
\]
Now,
\[
x^{1/2} = \sqrt{2}\sin\theta; \quad (2-x)^{1/2} = \sqrt{2}\cos\theta
\]
Also,
\[
x(2-x) = 2\sin^2\theta \cdot 2\cos^2\theta = 4\sin^2\theta\cos^2\theta = 4\sin^2\theta\cos^2\theta = [2\sin\theta\cos\theta]^2 = [\sin(2\theta)]^2
\]
Therefore,
\[
\sqrt{x(2-x)} = |\sin(2\theta)|
\]
On \([0, \pi/2]\), \(\sin(2\theta) \geq 0\), so no need for absolute value.

## Step 2: Change of Variables

Let’s compute the transformed integral:

\[
I = \int_{x=0}^{x=2} x^{1/2} (2-x)^{1/2} \cos(\sqrt{x(2-x)}) dx
\]
\[
= \int_{\theta=0}^{\theta=\frac{\pi}{2}} \left[\sqrt{2}\sin\theta\right] \left[\sqrt{2}\cos\theta\right] \cos(\sin(2\theta)) \cdot dx
\]
\[
= \int_0^{\frac{\pi}{2}} 2\sin\theta \cos\theta \cos(\sin(2\theta)) \cdot 2\sin(2\theta) d\theta
\]
But \(dx = 2\sin(2\theta)d\theta\), so
\[
x^{1/2}(2-x)^{1/2}dx = 2\sin\theta \cos\theta \cdot 2\sin(2\theta)d\theta
\]
But actually, the integrand is:
\[
2\sin\theta \cos\theta \cos(\sin(2\theta)) \cdot 2\sin(2\theta)d\theta = ?
\]

Wait, let's express in steps:
- \(x^{1/2} = \sqrt{2}\sin\theta\)
- \((2-x)^{1/2} = \sqrt{2}\cos\theta\)
- \(dx = 4\sin\theta\cos\theta d\theta = 2\sin(2\theta)d\theta\)
So,
\[
x^{1/2}(2-x)^{1/2}dx = (\sqrt{2}\sin\theta)(\sqrt{2}\cos\theta) \cdot 2\sin(2\theta)d\theta = 2\sin\theta\cos\theta \cdot 2\sin(2\theta)d\theta
\]
But \(2\sin\theta \cos\theta = \sin(2\theta)\),
So,
\[
= [\sin(2\theta)] \cdot [2\sin(2\theta)] d\theta = 2\sin^2(2\theta) d\theta
\]
So the integral becomes:
\[
I = \int_{0}^{\frac{\pi}{2}} 2\sin^2(2\theta) \cos(\sin(2\theta)) d\theta
\]

## Step 3: Further Simplification

Let \(u = 2\theta\), so \(d\theta = du/2\), as \(\theta\) goes from \(0\) to \(\frac{\pi}{2}\), \(u\) goes from \(0\) to \(\pi\).

Thus,
\[
I = \int_{0}^{\frac{\pi}{2}} 2\sin^2(2\theta) \cos(\sin(2\theta)) d\theta
\]
Let’s substitute:
\[
\sin^2(2\theta) = \sin^2(u)
\]
\[
\cos(\sin(2\theta)) = \cos(\sin u)
\]
So, \(d\theta = du/2\), thus:
\[
I = \int_{u=0}^{u=\pi} 2\sin^2(u)\cos(\sin u) \cdot \frac{du}{2}
\]
\[
= \int_{0}^{\pi} \sin^2 u \cos(\sin u) du
\]

## Step 4: Solving the New Integral

Let:
\[
J = \int_{0}^{\pi} \sin^2 u \cos(\sin u) du
\]

Let’s use the substitution \(t = \sin u\), so for \(u\) from \(0\) to \(\pi\), \(t\) goes from \(0\) to \(0\), but the function is symmetric, so let’s consider integrating by parts.

Alternatively, try integrating by parts directly:

Let’s take:
- \(f(u) = \sin^2 u\)
- \(g'(u) = \cos(\sin u)\)

Let’s consider another approach.

### Express \(\sin^2 u\) as \(\frac{1}{2}[1 - \cos(2u)]\):

So:
\[
J = \int_0^\pi \sin^2 u \cos(\sin u) du = \int_0^\pi \frac{1 - \cos(2u)}{2} \cos(\sin u) du = \frac{1}{2} \int_0^\pi \cos(\sin u) du - \frac{1}{2} \int_0^\pi \cos(2 u) \cos(\sin u) du
\]

Let us evaluate each term separately.

### First term: \(\int_0^\pi \cos(\sin u) du\)

This integral is known and related to Bessel functions:
\[
\int_0^\pi \cos(a \sin u) du = \pi J_0(a)
\]
So for \(a = 1\):
\[
\int_0^\pi \cos(\sin u) du = \pi J_0(1)
\]

### Second term: \(\int_0^\pi \cos(2u)\cos(\sin u) du\)

Use the identity:
\[
\cos(2u)\cos(\sin u) = \frac{1}{2}[\cos(\sin u + 2u) + \cos(\sin u - 2u)]
\]
But that will just complicate things, so instead, consider the Fourier-Bessel expansion.

Alternatively, recall the integral representation:
\[
\int_0^\pi \cos(nu) \cos(a \sin u) du = \pi J_n(a)
\]
So with \(n=2, a=1\):
\[
\int_0^\pi \cos(2u) \cos(\sin u) du = \pi J_2(1)
\]

### Summing Up

Thus,
\[
J = \frac{1}{2} \left[ \pi J_0(1) - \pi J_2(1) \right] = \frac{\pi}{2} [ J_0(1) - J_2(1) ]
\]

### Therefore, the original integral is

\[
I = J = \frac{\pi}{2} [ J_0(1) - J_2(1) ]
\]

## Step 5: Numerical Approximation

Let’s calculate \(J_0(1)\) and \(J_2(1)\) numerically.

- \(J_0(1) \approx 0.7651976866\)
- \(J_2(1) \approx 0.1149034849\)
- \(\pi/2 \approx 1.5707963268\)

So,
\[
I \approx \frac{\pi}{2}(0.7651976866 - 0.1149034849) \approx 1.5707963268 \times 0.6502942017 \approx 1.0218777974
\]

## Final Answers

- **Exact answer in LaTeX:** \(\frac{\pi}{2}\left[J_0(1) - J_2(1)\right]\)
- **Numerical approximation:** \(1.0218777974\)

```json
{"answer": "\\frac{\\pi}{2}\\left[J_0(1) - J_2(1)\\right]", "numerical_answer": "1.0218777974"}
```