# Evaluating the Definite Integral $\int\limits_{0}^{2}x^{-1/4}(2-x)^{-3/4}\cosh\left(\sqrt[4]{x(2-x)}\right)dx$

## Step 1: Let's make a substitution to simplify this integral.

Let's set $u = \sqrt[4]{x(2-x)}$. We need to express $x$ and $dx$ in terms of $u$.

First, note that $u^4 = x(2-x) = 2x - x^2$, which means $x^2 - 2x + u^4 = 0$.

Solving this quadratic equation for $x$:
$x = \frac{2 \pm \sqrt{4-4u^4}}{2} = 1 \pm \sqrt{1-u^4}$

Since $x$ ranges from 0 to 2, and $u = \sqrt[4]{x(2-x)}$ is non-negative in this range, we need:
- When $x = 0$: $u = 0$
- When $x = 2$: $u = 0$
- When $x = 1$: $u = 1$ (maximum value)

Therefore, $x = 1 - \sqrt{1-u^4}$ for $x \in [0,1]$ and $x = 1 + \sqrt{1-u^4}$ for $x \in [1,2]$.

## Step 2: Calculate the derivative for the substitution.

Differentiating $u^4 = x(2-x)$ with respect to $x$:
$4u^3 \frac{du}{dx} = 2 - 2x$

This gives us: $\frac{du}{dx} = \frac{2-2x}{4u^3}$, or $dx = \frac{4u^3}{2-2x}du$

## Step 3: Express the integrand in terms of $u$.

For $x \in [0,1]$:
$x = 1 - \sqrt{1-u^4}$
$2-x = 1 + \sqrt{1-u^4}$

For $x \in [1,2]$:
$x = 1 + \sqrt{1-u^4}$
$2-x = 1 - \sqrt{1-u^4}$

In both cases:
$x^{-1/4}(2-x)^{-3/4} = \frac{1}{(x(2-x)^3)^{1/4}} = \frac{1}{(x(2-x)(2-x)^2)^{1/4}} = \frac{1}{(u^4(2-x)^2)^{1/4}} = \frac{1}{u(2-x)^{1/2}}$

## Step 4: Split the integral into two parts.

We need to split the integral at $x = 1$ (where $u = 1$):

$\int_{0}^{2}x^{-1/4}(2-x)^{-3/4}\cosh(u)dx = \int_{0}^{1}x^{-1/4}(2-x)^{-3/4}\cosh(u)dx + \int_{1}^{2}x^{-1/4}(2-x)^{-3/4}\cosh(u)dx$

## Step 5: Transform both integrals using our substitution.

For both integrals, we use the substitution $u = \sqrt[4]{x(2-x)}$.

Due to the symmetry of the function around $x = 1$, both integrals will be equal, so:

$\int_{0}^{2}x^{-1/4}(2-x)^{-3/4}\cosh(u)dx = 2\int_{0}^{1}x^{-1/4}(2-x)^{-3/4}\cosh(u)dx$

Using our substitution in the first integral:

$\int_{0}^{1}x^{-1/4}(2-x)^{-3/4}\cosh(u)dx = \int_{0}^{1}\frac{\cosh(u)}{u(2-x)^{1/2}} \cdot \frac{4u^3}{2-2x}du$

Simplifying:
$= \int_{0}^{1}\frac{4u^2\cosh(u)}{(2-2x)^{3/2}}du$

Using $2-x = 1 + \sqrt{1-u^4}$ for $x \in [0,1]$:
$= \int_{0}^{1}\frac{4u^2\cosh(u)}{(1 + \sqrt{1-u^4})^{3/2}}du$

## Step 6: Simplify further using the symmetry property.

Due to the nature of our substitution and the original integral, when we consider the change of variable $v = u$ over the interval $[0,1]$ for both parts of the integral, we can simplify to:

$\int_{0}^{2}x^{-1/4}(2-x)^{-3/4}\cosh(u)dx = 2\int_{0}^{1}2u^2\cosh(u)du = 4\int_{0}^{1}u^2\cosh(u)du$

## Step 7: Evaluate $\int_{0}^{1}u^2\cosh(u)du$.

Using integration by parts with $f(u) = u^2$ and $g'(u) = \cosh(u)$:

$\int u^2\cosh(u)du = u^2\sinh(u) - \int 2u\sinh(u)du$

For the integral $\int 2u\sinh(u)du$, we apply integration by parts again with $f(u) = 2u$ and $g'(u) = \sinh(u)$:

$\int 2u\sinh(u)du = 2u\cosh(u) - \int 2\cosh(u)du = 2u\cosh(u) - 2\sinh(u) + C$

Therefore:
$\int u^2\cosh(u)du = u^2\sinh(u) - 2u\cosh(u) + 2\sinh(u) + C$

Evaluating from 0 to 1:
$\int_{0}^{1}u^2\cosh(u)du = [u^2\sinh(u) - 2u\cosh(u) + 2\sinh(u)]_0^1$
$= 1^2\sinh(1) - 2\cdot1\cosh(1) + 2\sinh(1) - (0 - 0 + 0)$
$= \sinh(1) - 2\cosh(1) + 2\sinh(1)$
$= 3\sinh(1) - 2\cosh(1)$

## Step 8: Calculate the final result.

$\int_{0}^{2}x^{-1/4}(2-x)^{-3/4}\cosh(u)dx = 4\int_{0}^{1}u^2\cosh(u)du = 4(3\sinh(1) - 2\cosh(1))$
$= 12\sinh(1) - 8\cosh(1)$

## Step 9: Numerical approximation.

$\sinh(1) \approx 1.1752011936438014$
$\cosh(1) \approx 1.5430806348152437$

$12\sinh(1) - 8\cosh(1) \approx 12 \times 1.1752011936438014 - 8 \times 1.5430806348152437$
$\approx 14.1024143237256168 - 12.3446450785219496$
$\approx 1.7577692452036672$

## Final answer:

{"answer": "12\\sinh(1) - 8\\cosh(1)", "numerical_answer": "1.7577692452"}