<think>
Okay, so I need to solve the definite integral from 0 to 2 of x^(-1/4) times (2 - x)^(-3/4) times cosh(1 times the fourth root of x(2 - x)) dx. Hmm, let's break this down step by step. 

First, the integrand looks a bit complicated with those negative exponents and the hyperbolic cosine function. The exponents on x and (2 - x) are -1/4 and -3/4, respectively. The argument inside the cosh is the fourth root of x(2 - x). Maybe there's a substitution that can simplify this expression.

Let me think about substitution. The term inside the cosh is the fourth root of x(2 - x). Let's denote t = [x(2 - x)]^(1/4). Then t^4 = x(2 - x). But I'm not sure if that's helpful yet. Alternatively, maybe a substitution that simplifies the product x(2 - x). Let's see, if I let u = x/(2 - x), but I'm not sure. Alternatively, maybe a trigonometric substitution?

Wait, the limits of integration are from 0 to 2. The expression x(2 - x) is symmetric around x = 1, and it's a quadratic that peaks at x=1. Maybe a substitution like x = 2 sin^2 θ or something similar. Let's try that. Let me set x = 2 sin^2 θ. Then when x=0, θ=0, and when x=2, θ=π/2. Let's compute dx: dx = 4 sin θ cos θ dθ. Then (2 - x) = 2 - 2 sin^2 θ = 2 cos^2 θ. So x(2 - x) = 2 sin^2 θ * 2 cos^2 θ = 4 sin^2 θ cos^2 θ. Then the fourth root of that would be sqrt(sin θ cos θ). Wait, the fourth root of 4 sin^2 θ cos^2 θ is (4)^(1/4) * (sin θ cos θ)^(1/2). But 4^(1/4) is sqrt(2). So the argument inside cosh becomes sqrt(2) * sqrt(sin θ cos θ). Hmm, not sure if that helps.

But let's proceed with substitution x = 2 sin^2 θ. Then, substituting into the integral:

Original integral becomes:

∫ from θ=0 to θ=π/2 of [ (2 sin^2 θ)^(-1/4) * (2 cos^2 θ)^(-3/4) ) * cosh( sqrt(2) sqrt(sin θ cos θ) ) ] * 4 sin θ cos θ dθ.

Let's simplify the terms:

First, (2 sin^2 θ)^(-1/4) = 2^(-1/4) sin^(-1/2) θ

Similarly, (2 cos^2 θ)^(-3/4) = 2^(-3/4) cos^(-3/2) θ

Multiply those together: 2^(-1/4 - 3/4) sin^(-1/2) θ cos^(-3/2) θ = 2^(-1) sin^(-1/2) θ cos^(-3/2) θ = (1/2) sin^(-1/2) θ cos^(-3/2) θ

Then, the rest of the integrand is cosh( sqrt(2) sqrt(sin θ cos θ) ) * 4 sin θ cos θ dθ.

So putting it all together:

Integral) (1/2) * 4 * sin^(-1/2) θ cos^(-3/2) θ * sin θ cos θ * cosh( sqrt(2) sqrt(sin θ cos θ) ) dθ

Simplify the coefficients: (1/2)*4 = 2

Now, the terms with sin and cos:

sin^(-1/2) θ * sin θ = sin^(1 - 1/2) θ = sin^(1/2) θ

cos^(-3/2) θ * cos θ = cos^(-3/2 + 1) θ = cos^(-1/2) θ

So now the integrand becomes:

2 * sin^(1/2) θ * cos^(-1/2) θ * cosh( sqrt(2) sqrt(sin θ cos θ) ) dθ

Hmm, so 2 * sqrt(sin θ) / sqrt(cos θ) * cosh( sqrt(2) sqrt(sin θ cos θ) ) dθ

Let me write sqrt(sin θ cos θ) as sqrt(sin θ) * sqrt(cos θ). So sqrt(2) * sqrt(sin θ) * sqrt(cos θ) = sqrt(2) * sqrt(sin θ cos θ). Wait, but inside the cosh, it's sqrt(2) times sqrt(sin θ cos θ). Let me denote u = sqrt(sin θ cos θ). Then the argument of cosh is sqrt(2) u.

But maybe another substitution here. Let's set t = sqrt(sin θ / cos θ). Then t^2 = sin θ / cos θ, so sin θ = t^2 cos θ. Then using sin^2 θ + cos^2 θ = 1, we get t^4 cos^2 θ + cos^2 θ = 1 => cos^2 θ (t^4 + 1) = 1 => cos θ = 1 / sqrt(t^4 + 1). Hmm, not sure if that's helpful.

Alternatively, let's consider substituting u = sqrt(sin θ cos θ). Let me compute u:

u = sqrt(sin θ cos θ) = (sin θ cos θ)^(1/2). Let's compute du/dθ:

du/dθ = (1/2)(sin θ cos θ)^(-1/2) [cos^2 θ - sin^2 θ] dθ

Hmm, but that might complicate things. Alternatively, maybe set t = sqrt(2) u = sqrt(2) sqrt(sin θ cos θ). Then t = sqrt(2 sin θ cos θ) = sqrt(sin 2θ). Wait, since sin 2θ = 2 sin θ cos θ, so sqrt(sin 2θ) = sqrt(2 sin θ cos θ). So t = sqrt(sin 2θ). Then, when θ=0, t=0, and when θ=π/2, t=sqrt(sin π)=0. Wait, but θ goes from 0 to π/2, so 2θ goes from 0 to π, so sin 2θ goes from 0 up to 1 and back to 0. Hmm, but integrating from t=0 to t=1 and back to t=0. That might not be helpful. Maybe another substitution.

Wait, let's look back at the integrand after substitution:

2 * sqrt(sin θ) / sqrt(cos θ) * cosh( sqrt(2) sqrt(sin θ cos θ) ) dθ

Let me write sqrt(sin θ)/sqrt(cos θ) as sqrt(tan θ). So sqrt(tan θ) = sqrt(sin θ / cos θ). So the integrand becomes 2 * sqrt(tan θ) * cosh( sqrt(2) * sqrt(sin θ cos θ) ) dθ.

But sqrt(sin θ cos θ) is sqrt( (sin θ cos θ) ). Let's note that sin θ cos θ = (1/2) sin 2θ. So sqrt(sin θ cos θ) = sqrt( (1/2) sin 2θ ) = (1/√2) sqrt(sin 2θ). Therefore, the argument inside cosh becomes sqrt(2) * (1/√2) sqrt(sin 2θ) = sqrt(sin 2θ). So the integrand simplifies to 2 * sqrt(tan θ) * cosh( sqrt(sin 2θ) ) dθ.

Hmm, that's a bit simpler. So now the integral is:

2 ∫ sqrt(tan θ) * cosh( sqrt(sin 2θ) ) dθ from θ=0 to θ=π/2.

But I'm not sure if this helps. Maybe another substitution. Let's try substituting φ = 2θ. Then when θ=0, φ=0; θ=π/2, φ=π. Then dφ = 2 dθ, so dθ = dφ/2. The integral becomes:

2 ∫ sqrt(tan(φ/2)) * cosh( sqrt(sin φ) ) * (dφ/2) from φ=0 to φ=π.

So that's ∫ sqrt(tan(φ/2)) * cosh( sqrt(sin φ) ) dφ from 0 to π. Hmm, not sure if that's better.

Alternatively, maybe consider a substitution that can relate to the argument of the cosh. Let's see, the argument is sqrt(sin 2θ). Let me set t = sqrt(sin 2θ). Then t^2 = sin 2θ. Differentiating both sides: 2t dt = 2 cos 2θ dθ => t dt = cos 2θ dθ. Hmm, but then we need to express cos 2θ in terms of t. Since sin 2θ = t^2, cos 2θ = sqrt(1 - t^4). Wait, but 2θ ranges from 0 to π, so 2θ ranges from 0 to 2π. But when θ is from 0 to π/2, 2θ is from 0 to π, so cos2θ would be from 1 to -1. So sqrt(1 - t^4) would be valid only when cos2θ is positive, i.e., 0 ≤ 2θ ≤ π/2, so θ from 0 to π/4. But from π/4 to π/2, cos2θ is negative, so sqrt(1 - t^4) would be imaginary. Hmm, this complicates things. Maybe this substitution isn't the way to go.

Let me think differently. The original integral is from 0 to 2. The integrand is x^{-1/4} (2 - x)^{-3/4} cosh( [x(2 - x)]^{1/4} ). Let me check if this is related to a Beta function or Gamma function. The Beta function is ∫0^1 t^{c-1} (1 - t)^{d -1} dt, which is related to Gamma functions. But here, the integral is from 0 to 2, and the exponents are -1/4 and -3/4. Also, the presence of the cosh complicates things. But maybe if we can express cosh in terms of a series expansion, then integrate term by term.

Let's recall that cosh(z) = Σ_{n=0}^∞ z^{2n}/(2n)! So maybe expanding the cosh term as a power series and then integrating term by term. Let's try that.

So, cosh( [x(2 - x)]^{1/4} ) = Σ_{n=0}^∞ [x(2 - x)]^{n/2}/(2n)! )

Therefore, the integral becomes:

Σ_{n=0}^∞ [1/(2n)!] ∫0^2 x^{-1/4} (2 - x)^{-3/4} [x(2 - x)]^{n/2} dx

Simplify the integrand:

x^{-1/4} (2 - x)^{-3/4} * x^{n/2} (2 - x)^{n/2} = x^{n/2 - 1/4} (2 - x)^{n/2 - 3/4}

So the integral is:

Σ_{n=0}^∞ [1/(2n)!] ∫0^2 x^{n/2 - 1/4} (2 - x)^{n/2 - 3/4} dx

Now, this integral looks like a Beta function. Let's recall that ∫0^a x^{c - 1} (a - x)^{d - 1} dx = a^{c + d - 1} B(c, d) = a^{c + d - 1} Γ(c)Γ(d)/Γ(c + d)

In our case, a = 2, c = n/2 - 1/4 + 1 = n/2 + 3/4? Wait, no. Wait, the integral is ∫0^a x^{c - 1} (a - x)^{d - 1} dx. So in our case, x^{n/2 - 1/4} (2 - x)^{n/2 - 3/4} = x^{c - 1} (2 - x)^{d - 1} where c = n/2 - 1/4 + 1 = n/2 + 3/4? Wait, no. Wait, c - 1 = n/2 - 1/4 => c = n/2 - 1/4 + 1 = n/2 + 3/4. Similarly, d - 1 = n/2 - 3/4 => d = n/2 - 3/4 + 1 = n/2 + 1/4.

Therefore, the integral becomes:

2^{c + d - 1} Γ(c) Γ(d) / Γ(c + d) = 2^{(n/2 + 3/4) + (n/2 + 1/4) - 1} Γ(n/2 + 3/4) Γ(n/2 + 1/4) / Γ(n + 1)

Simplify the exponent of 2:

(n/2 + 3/4) + (n/2 + 1/4) - 1 = n + 1 - 1 = n - 0. So 2^{n - 1} ?

Wait, let's compute:

c + d - 1 = (n/2 + 3/4) + (n/2 + 1/4) - 1 = n + 1) -1 = n. So 2^{n} ?

Wait, no. Wait, the formula is a^{c + d - 1} where a=2. So c + d -1 = (n/2 + 3/4) + (n/2 + 1/4) -1 = n + 1 -1 = n. Therefore, 2^{n} Γ(n/2 + 3/4) Γ(n/2 + 1/4) / Γ(n + 1)

Therefore, the integral over x is 2^{n} Γ(n/2 + 3/4) Γ(n/2 + 1/4) / Γ(n + 1)

Therefore, the original series becomes:

Σ_{n=0}^∞ [1/(2n)!] * 2^{n} Γ(n/2 + 3/4) Γ(n/2 + 1/4) / Γ(n + 1)

Hmm, this seems complicated, but maybe there's a way to simplify this series. Let's recall some properties of the Gamma function. For example, the duplication formula or some relation that connects Γ(n/2 + 3/4) and Γ(n/2 + 1/4). 

Alternatively, perhaps using the reflection formula or beta function properties. Alternatively, note that Γ(z)Γ(1 - z) = π / sin(π z). But here, the arguments are n/2 + 3/4 and n/2 + 1/4. Let's check if they sum to something. Let's compute (n/2 + 3/4) + (n/2 + 1/4) = n + 1. So their sum is n + 1. So Γ(n/2 + 3/4) Γ(n/2 + 1/4) = Γ(a) Γ(b) where a + b = n + 1. Hmm, not sure if that helps.

Alternatively, maybe express Γ(n/2 + 3/4) Γ(n/2 + 1/4) using the duplication formula. The duplication formula is Γ(z)Γ(z + 1/2) = 2^{1 - 2z} sqrt(π) Γ(2z). Let's see if that can be applied here. Let me set z = n/2 + 1/4. Then Γ(z) Γ(z + 1/2) = Γ(n/2 + 1/4) Γ(n/2 + 3/4) = 2^{1 - 2(n/2 + 1/4)} sqrt(π) Γ(2(n/2 + 1/4)) = 2^{1 - n - 1/2} sqrt(π) Γ(n + 1/2) = 2^{-n + 1/2} sqrt(π) Γ(n + 1/2)

Therefore, Γ(n/2 + 3/4) Γ(n/2 + 1/4) = 2^{-n + 1/2} sqrt(π) Γ(n + 1/2)

So substituting back into the series:

Σ_{n=0}^∞ [1/(2n)!] * 2^{n} * [2^{-n + 1/2} sqrt(π) Γ(n + 1/2)] / Γ(n + 1)

Simplify the powers of 2: 2^{n} * 2^{-n + 1/2} = 2^{1/2} = sqrt(2)

So the series becomes:

sqrt(2) sqrt(π) Σ_{n=0}^∞ [1/(2n)!] * Γ(n + 1/2) / Γ(n + 1)

But Γ(n + 1) = n! and Γ(n + 1/2) = (2n)! sqrt(π) / 4^n n! ) from the double factorial relation. Wait, Γ(n + 1/2) = (2n)! / (4^n n!) ) sqrt(π). Let me confirm:

Yes, Γ(n + 1/2) = (2n)! / (4^n n!) ) sqrt(π). So substituting that in:

Γ(n + 1/2) = (2n)! sqrt(π) / (4^n n! )

Therefore, the term inside the series becomes:

[1/(2n)!] * [ (2n)! sqrt(π) / (4^n n! ) ) ] / n! ) = [1/(2n)!] * (2n)! sqrt(π) / (4^n n!^2) ) = sqrt(π) / (4^n n!^2 )

Therefore, the series is:

sqrt(2) sqrt(π) * Σ_{n=0}^∞ sqrt(π) / (4^n n!^2 )

Wait, let's compute:

The entire coefficient is sqrt(2) sqrt(π) multiplied by sqrt(π) / (4^n n!^2 )

So sqrt(2) * π * Σ_{n=0}^∞ 1 / (4^n n!^2 )

But Σ_{n=0}^∞ 1 / (4^n n!^2 ) is the modified Bessel function of the first kind I_0(1). Wait, because I_0(z) = Σ_{n=0}^∞ (z/2)^{2n} / (n!^2 ). So if we set z = 1, then I_0(1) = Σ_{n=0}^∞ (1/2)^{2n} / (n!^2 ) = Σ_{n=0}^∞ 1/(4^n n!^2 )

Therefore, the series Σ_{n=0}^∞ 1/(4^n n!^2 ) = I_0(1)

Therefore, the original integral becomes sqrt(2) * π * I_0(1)

Wait, let's check:

sqrt(2) * sqrt(π) * sqrt(π) * Σ_{n=0}^∞ 1/(4^n n!^2 ) = sqrt(2) * π * I_0(1)

Yes, because sqrt(π) * sqrt(π) = π.

So the integral is sqrt(2) π I_0(1)

But wait, the modified Bessel function I_0(1) is a known constant. So the exact answer is sqrt(2) π I_0(1). But can we express this in terms of more elementary functions? Probably not, since I_0 is a special function. So the exact answer is sqrt(2) π times the modified Bessel function of the first kind of order 0 evaluated at 1.

But let me verify the steps again to make sure I didn't make a mistake. Starting from the substitution, expanding the cosh as a series, then integrating term by term using the Beta function, applying the duplication formula, and recognizing the series as I_0(1). Seems correct.

Alternatively, maybe there's a substitution that can directly relate the integral to the Bessel function. But given the steps above, the result seems to be sqrt(2) π I_0(1).

Now, the numerical approximation. I_0(1) is approximately 1.266065878. Let's compute sqrt(2) * π * 1.266065878.

First, sqrt(2) ≈ 1.41421356237

π ≈ 3.1415926535

Multiply them: 1.41421356237 * 3.1415926535 ≈ 4.442882908

Then multiply by I_0(1) ≈ 1.266065878:

4.442882908 * 1.266065878 ≈ Let's compute this:

4 * 1.266 = 5.064

0.442882908 * 1.266 ≈ 0.442882908 * 1 = 0.442882908, 0.442882908 * 0.266 ≈ 0.1178. So total ≈ 0.442882908 + 0.1178 ≈ 0.5606. So total approx 5.064 + 0.5606 ≈ 5.6246. But let's compute more accurately:

4.442882908 * 1.266065878:

First, 4 * 1.266065878 = 5.064263512

0.442882908 * 1.266065878:

Compute 0.4 * 1.266065878 = 0.5064263512

0.04 * 1.266065878 = 0.0506426351

0.002882908 * 1.266065878 ≈ 0.00365

Adding up: 0.5064263512 + 0.0506426351 = 0.5570689863 + 0.00365 ≈ 0.5607189863

Total: 5.064263512 + 0.5607189863 ≈ 5.6249824983

So approximately 5.6249824983. Rounded to 10 decimal places, that's 5.6249824983. Let me check with a calculator:

Using precise values:

I_0(1) ≈ 1.2660658777520084

sqrt(2) ≈ 1.4142135623730951

π ≈ 3.141592653589793

So sqrt(2) * π ≈ 1.4142135623730951 * 3.141592653589793 ≈ 4.442882908158368

Then 4.442882908158368 * 1.2660658777520084 ≈ 

Let's compute 4 * 1.2660658777520084 = 5.0642635101008034

0.442882908158368 * 1.2660658777520084:

Breakdown:

0.4 * 1.2660658777520084 = 0.5064263511008034

0.04 * 1.2660658777520084 = 0.05064263511008034

0.002882908158368 * 1.2660658777520084 ≈ 0.00365 (exact value: 0.002882908158368 * 1.2660658777520084 ≈ 0.00365)

Adding up: 0.5064263511008034 + 0.05064263511008034 = 0.5570689862108838 + 0.00365 ≈ 0.5607189862108838

Total: 5.0642635101008034 + 0.5607189862108838 ≈ 5.624982496311687

So approximately 5.6249824963, which rounds to 5.6249824963. To 10 decimal places, 5.6249824963.

But let me check with a calculator for more precision. Alternatively, use known values:

I_0(1) ≈ 1.2660658777520084

Multiply by sqrt(2) * π:

sqrt(2) * π ≈ 4.442882908158368

4.442882908158368 * 1.2660658777520084 ≈ 

Let's compute:

4 * 1.2660658777520084 = 5.0642635101008034

0.442882908158368 * 1.2660658777520084:

Compute 0.4 * 1.2660658777520084 = 0.5064263511008034

0.04 * 1.2660658777520084 = 0.05064263511008034

0.002882908158368 * 1.2660658777520084 ≈ 0.002882908158368 * 1.2660658777520084 ≈ 0.00365 (exact calculation: 0.002882908158368 * 1.2660658777520084 ≈ 0.00365)

Adding up: 0.5064263511008034 + 0.05064263511008034 = 0.5570689862108838 + 0.00365 ≈ 0.5607189862108838

Total: 5.0642635101008034 + 0.5607189862108838 ≈ 5.624982496311687

So approximately 5.6249824963. Rounded to 10 decimal places, 5.6249824963. But let me check with a calculator:

Using Wolfram Alpha, the integral ∫_{0}^{2} x^{-1/4} (2 - x)^{-3/4} cosh( (x(2 - x))^{1/4} ) dx.

But since I can't access external resources, but according to the steps, the exact answer is sqrt(2) π I_0(1), and the numerical value is approximately 5.6249824963.

Therefore, the exact answer is \sqrt{2} \pi I_0(1), and the numerical approximation is approximately 5.6249824963, which rounds to 5.6249824963 when rounded to 10 decimal places.

But let me check if there's a different approach. For example, maybe the substitution t = x/2, so x = 2t, dx = 2dt. Then the integral becomes:

∫0^1 (2t)^{-1/4} (2 - 2t)^{-3/4} cosh( (2t(2 - 2t))^{1/4} ) * 2 dt

Simplify:

(2^{-1/4} t^{-1/4}) * (2^{-3/4} (1 - t)^{-3/4}) * 2 * cosh( (4t(1 - t))^{1/4} ) dt

Combine the constants:

2^{-1/4 -3/4} * 2 = 2^{-1} * 2 = 1/2 * 2 = 1

So the integral becomes:

∫0^1 t^{-1/4} (1 - t)^{-3/4} cosh( (4t(1 - t))^{1/4} ) dt

But (4t(1 - t))^{1/4} = (4)^{1/4} (t(1 - t))^{1/4} = sqrt(2) (t(1 - t))^{1/4}

So the integral is:

∫0^1 t^{-1/4} (1 - t)^{-3/4} cosh( sqrt(2) (t(1 - t))^{1/4} ) dt

But this seems similar to the original integral but scaled. Not sure if this helps. However, this substitution shows that the integral is equal to the original one, which is expected.

Alternatively, perhaps another substitution. Let me set u = t(1 - t). Then du/dt = 1 - 2t. But this might not help.

Alternatively, maybe set v = (t(1 - t))^{1/4}, but this complicates differentiation.

Alternatively, note that the integral after substitution is similar to a Beta function form, but with the cosh term. However, we already expanded the cosh as a series and arrived at the expression involving the Bessel function. So I think the steps are correct.

Therefore, the exact answer is sqrt(2) π I_0(1), and the numerical value is approximately 5.6249824963.
</think>

{"answer": "\\sqrt{2} \\pi I_{0}(1)", "numerical_answer": 5.6249824963}