We wish to evaluate
  I = ∫₀^(π/2) min{sin x, cot x} dx.

Step 1. Determine the splitting point.
For x in (0, π/2) the functions behave as follows:
 • sin x is increasing from 0 to 1,
 • cot x is decreasing from +∞ to 0.
Thus, for very small x we have sin x < cot x while for x near π/2 we have cot x < sin x. Their “switch” occurs when
  sin x = cot x.
Since cot x = cos x/sin x (for x in (0, π/2)), equate
  sin x = cos x/sin x ⟹ sin² x = cos x.
This equation can be rewritten (using sin² x = 1 − cos² x) as
  1 − cos² x = cos x ⟹ cos² x + cos x − 1 = 0.
The unique solution in [0, π/2] is
  cos x₀ = (√5 − 1)/2.
Thus, the splitting point is x₀ = arccos((√5 − 1)/2).

Step 2. Write the integral as two parts.
On [0, x₀] we have sin x ≤ cot x so that min{sin x, cot x} = sin x.
On [x₀, π/2] we have cot x ≤ sin x so that min{sin x, cot x} = cot x.
Thus,
  I = ∫₀^(x₀) sin x dx + ∫_(x₀)^(π/2) cot x dx.

Step 3. Evaluate each integral.

(a) Evaluate ∫ sin x dx:
  ∫ sin x dx = −cos x + C.
Thus,
  ∫₀^(x₀) sin x dx = [−cos x]₀^(x₀) = (−cos x₀) − (−cos 0)
          = 1 − cos x₀.

(b) Evaluate ∫ cot x dx:
Recall, ∫ cot x dx = ln|sin x| + C.
Thus,
  ∫_(x₀)^(π/2) cot x dx = [ln sin x]_(x₀)^(π/2)
             = ln(sin(π/2)) − ln(sin x₀)
             = 0 − ln(sin x₀) = −ln(sin x₀).

So,
  I = (1 − cos x₀) − ln(sin x₀).

Step 4. Express the answer exactly.
We already know
  cos x₀ = (√5 − 1)/2.
Also, since sin² x₀ = cos x₀ from the equation sin² x₀ = cos x₀, we have
  sin x₀ = √(cos x₀) = √((√5 − 1)/2).
Thus, the answer becomes
  I = 1 − (√5 − 1)/2 − ln(√((√5 − 1)/2)).
Notice that ln(√A) = (1/2) ln A. Hence,
  I = 1 − (√5 − 1)/2 − (1/2) ln((√5 − 1)/2).

Sometimes it is preferable to express the answer in terms of the golden ratio, φ = (1 + √5)/2, using the fact that
  1/φ = (√5 − 1)/2.
Then,
  I = 1 − 1/φ − (1/2) ln(1/φ)
    = 1 − 1/φ + (1/2) ln φ.
Also, 1 − 1/φ can be written as
  1 − 1/φ = (φ − 1)/φ.
But one acceptable answer in closed‐form is
  I = (3 − √5)/2 + (1/2) ln((1 + √5)/2).
To see this, note:
  1 − (√5 − 1)/2 = (2 − √5 + 1)/2 = (3 − √5)/2,
and ln((1 + √5)/2) = ln φ.

Thus the exact answer is

  I = (3 − √5)/2 + (1/2) ln((1 + √5)/2).

Step 5. Compute a numerical approximation.
Using approximate values:
 √5 ≈ 2.2360679775 so that
  (3 − √5)/2 ≈ (3 − 2.2360679775)/2 ≈ 0.3819660113.
Also, (1 + √5)/2 ≈ 1.6180339888 and ln(1.6180339888) ≈ 0.4812118251, hence
  (1/2) ln((1 + √5)/2) ≈ 0.2406059126.
Therefore,
  I ≈ 0.3819660113 + 0.2406059126 = 0.6225719239.

Thus, the final answers are:

Exact answer: I = (3 − √5)/2 + (1/2) ln((1 + √5)/2)
Numerical approximation: 0.6225719239

{"answer": "$(3-\\sqrt{5})/2+\\frac{1}{2}\\ln((1+\\sqrt{5})/2)$", "numerical_answer": "0.6225719239"}