Let's evaluate the integral:
\[
I = \int_0^{2} x^{1.0-3/2}(2.0-x)^{1.0-1/2} [1-0.5x(2.0-x)]^{-1.0}\, dx
\]

First, let's simplify the exponents:
- \(1.0 - 3/2 = -0.5\)
- \(1.0 - 1/2 = 0.5\)

So the integral becomes:
\[
I = \int_0^{2} x^{-0.5} (2-x)^{0.5} \left[1-0.5x(2-x)\right]^{-1}\, dx
\]

Let's simplify the term inside the brackets:
\[
1 - 0.5 x (2-x) = 1 - 0.5 (2x - x^2) = 1 - x + 0.5 x^2
\]

So:
\[
I = \int_0^{2} x^{-0.5} (2-x)^{0.5} \left[1 - x + 0.5 x^2\right]^{-1}\, dx
\]

Let’s try the substitution \(x = 2t\), so as \(x\) goes from \(0\) to \(2\), \(t\) goes from \(0\) to \(1\):

- \(x = 2t\)
- \(dx = 2 dt\)
- \(x^{-0.5} = (2t)^{-0.5} = 2^{-0.5} t^{-0.5}\)
- \((2-x)^{0.5} = (2-2t)^{0.5} = 2^{0.5}(1-t)^{0.5}\)
- \(1 - x + 0.5 x^2 = 1 - 2t + 0.5 (4t^2) = 1 - 2t + 2t^2\)

Put these into the integral:
\[
I = \int_{t=0}^{1} \left[2^{-0.5} t^{-0.5}\right] \left[2^{0.5} (1-t)^{0.5}\right] \left[1-2t+2t^2\right]^{-1} \cdot 2 dt
\]

\(2^{-0.5} \cdot 2^{0.5} = 1\), so:
\[
I = 2 \int_0^1 t^{-0.5} (1-t)^{0.5} \left[1-2t+2t^2\right]^{-1} dt
\]

Now, let's factor \(1-2t+2t^2\):

Completing the square:
\[
1-2t+2t^2 = 2(t^2 - t) + 1 = 2\left(t^2 - t + \frac{1}{4}\right) + 1 - \frac{1}{2}
= 2\left(t-\frac{1}{2}\right)^2 + \frac{1}{2}
\]

Or, just keep it as is for now.

This integral fits the Appell hypergeometric function case:
Recall that
\[
\int_{0}^{1} t^{c-1} (1-t)^{d-1} (1-ut)^{-a} (1-vt)^{-b} dt = \frac{\Gamma(c)\Gamma(d)}{\Gamma(c+d)} F_1(a, b, c; c+d; u, v)
\]
But our denominator is a quadratic, not linear.

Alternatively, notice that
\[
\frac{1}{1 - 2t + 2t^2} = \frac{1}{2(t^2 - t + 0.5)}
\]

Alternatively, recall the following beta integral involving a quadratic factor: For \(\alpha, \beta > -1\):
\[
\int_0^1 t^{\alpha}(1-t)^{\beta}(1 - at + b t^2)^{-s} dt = \text{can be expressed in terms of hypergeometric or Appell functions}
\]
Specifically, see Gradshteyn & Ryzhik 3.259.3:
\[
\int_0^1 t^{\mu-1} (1-t)^{\nu-1} (1 - 2a t + b t^2)^{-\lambda} dt = B(\mu, \nu) \, _2F_1\left(\lambda, \mu; \mu+\nu; \frac{1 - a}{1 - a + b}\right) (1 - a + b)^{-\lambda}
\]
But we need it in form \(1-2t+2t^2\).
Let’s write \(1-2t+2t^2 = 2(t^2-t+0.5)\).

Let’s transform as follows:

Let’s try expressing the integral in terms of the beta and hypergeometric function.

In Gradshteyn & Ryzhik 3.259.3, the integral is:
\[
\int_0^1 t^{\mu-1} (1-t)^{\nu-1} (1 - 2a t + b t^2)^{-\lambda} dt = B(\mu, \nu) \; _2F_1\left(\lambda, \mu; \mu+\nu; \frac{1 - a}{1 - a + b}\right) (1 - a + b)^{-\lambda}
\]
where \(B(\mu, \nu) = \frac{\Gamma(\mu)\Gamma(\nu)}{\Gamma(\mu+\nu)}\)

For our case,
- \(\mu = 0.5\)
- \(\nu = 1.5\)
- \(\lambda = 1\)
- \(a = 1\)
- \(b = 2\)

So:
- \(B(\mu, \nu) = \frac{\Gamma(0.5)\Gamma(1.5)}{\Gamma(2)}\)
- \(1-a = 0\)
- \(1-a+b = 0+2=2\)
- \(\frac{1-a}{1-a+b} = 0\)
- \((1-a+b)^{-\lambda} = 2^{-1} = \frac{1}{2}\)

Therefore,
\[
I = 2 \int_0^1 t^{-0.5} (1-t)^{0.5} (1 - 2t + 2t^2)^{-1} dt
= 2 \left( B(0.5, 1.5) \cdot \phantom{}_2F_1\left(1, 0.5; 2; 0 \right) \cdot \frac{1}{2} \right)
\]

But, \( _2F_1(1,0.5;2;0) = 1 \) (because \( _2F_1(a,b;c;0) = 1 \)).

\(B(0.5,1.5) = \frac{\Gamma(0.5)\Gamma(1.5)}{\Gamma(2)}\).

Recall:

- \(\Gamma(0.5) = \sqrt{\pi}\)
- \(\Gamma(1.5) = \frac{1}{2}\sqrt{\pi}\)
- \(\Gamma(2) = 1!\) \(= 1\)

So:
\[
B(0.5, 1.5) = \sqrt{\pi} \cdot \frac{1}{2}\sqrt{\pi} = \frac{\pi}{2}
\]

Combine everything:
\[
I = 2 \cdot \left( \frac{\pi}{2} \cdot 1 \cdot \frac{1}{2} \right ) = 2 \cdot \frac{\pi}{4} = \frac{\pi}{2}
\]

**Numerical approximation:**
\[
\frac{\pi}{2} \approx 1.5707963268
\]

**Final answer:**
```json
{"answer": "\\frac{\\pi}{2}", "numerical_answer": "1.5707963268"}
```