To compute the definite integral \(\int_0^1 \left( (1 - x^{25})^{1/20} - (1 - x^{20})^{1/25} \right) \, dx\), we follow these steps:

1. **Analytical Computation**:
   - Denote the integrals separately:
     \[
     I_1 = \int_0^1 (1 - x^{25})^{1/20} \, dx \quad \text{and} \quad I_2 = \int_0^1 (1 - x^{20})^{1/25} \, dx
     \]
   - Use substitution to express each integral in terms of the Beta function \(B(a, b)\):
     - For \(I_1\), let \(u = x^{25}\), leading to:
       \[
       I_1 = \frac{1}{25} B\left( \frac{1}{25}, \frac{21}{20} \right)
       \]
     - For \(I_2\), let \(v = x^{20}\), leading to:
       \[
       I_2 = \frac{1}{20} B\left( \frac{1}{20}, \frac{26}{25} \right)
       \]
   - Convert Beta functions to Gamma functions using \(B(a, b) = \frac{\Gamma(a)\Gamma(b)}{\Gamma(a + b)}\):
     - For \(I_1\):
       \[
       I_1 = \frac{1}{25} \cdot \frac{\Gamma\left( \frac{1}{25} \right) \Gamma\left( \frac{21}{20} \right)}{\Gamma\left( \frac{109}{100} \right)}
       \]
     - For \(I_2\):
       \[
       I_2 = \frac{1}{20} \cdot \frac{\Gamma\left( \frac{1}{20} \right) \Gamma\left( \frac{26}{25} \right)}{\Gamma\left( \frac{109}{100} \right)}
       \]
   - Simplify using properties of the Gamma function \(\Gamma(z+1) = z\Gamma(z)\):
     - \(\Gamma\left( \frac{21}{20} \right) = \frac{1}{20} \Gamma\left( \frac{1}{20} \right)\)
     - \(\Gamma\left( \frac{26}{25} \right) = \frac{1}{25} \Gamma\left( \frac{1}{25} \right)\)
   - Substitute these back into the expressions for \(I_1\) and \(I_2\), showing they are equal:
     \[
     I_1 = I_2
     \]
   - Therefore, the integral \(I_1 - I_2 = 0\).

2. **Numerical Approximation**:
   - The numerical approximation of the result is \(0.0000000000\).

### Final Answer
{"answer": "0", "numerical_answer": "0.0000000000"}