Let's compute the definite integral step by step:

\[
\int_0^6 \left( x + (x-3)^7 + \sin(x-3) \right) dx
\]

### Step 1: Break the integral into parts
The integral can be split into three separate integrals:

\[
\int_0^6 x \, dx + \int_0^6 (x-3)^7 \, dx + \int_0^6 \sin(x-3) \, dx
\]

### Step 2: Compute each integral separately

1. **First integral:**
\[
\int x \, dx = \frac{x^2}{2} + C
\]
Evaluated from 0 to 6:
\[
\left. \frac{x^2}{2} \right|_0^6 = \frac{6^2}{2} - \frac{0^2}{2} = 18 - 0 = 18
\]

2. **Second integral:**
Let \( u = x - 3 \), then \( du = dx \). The integral becomes:
\[
\int (x-3)^7 \, dx = \int u^7 \, du = \frac{u^8}{8} + C = \frac{(x-3)^8}{8} + C
\]
Evaluated from 0 to 6:
\[
\left. \frac{(x-3)^8}{8} \right|_0^6 = \frac{(6-3)^8}{8} - \frac{(0-3)^8}{8} = \frac{3^8}{8} - \frac{(-3)^8}{8} = \frac{6561}{8} - \frac{6561}{8} = 0
\]

3. **Third integral:**
Let \( u = x - 3 \), then \( du = dx \). The integral becomes:
\[
\int \sin(x-3) \, dx = \int \sin u \, du = -\cos u + C = -\cos(x-3) + C
\]
Evaluated from 0 to 6:
\[
\left. -\cos(x-3) \right|_0^6 = -\cos(6-3) - (-\cos(0-3)) = -\cos(3) + \cos(-3)
\]
Since \( \cos(-3) = \cos(3) \), this simplifies to:
\[
-\cos(3) + \cos(3) = 0
\]

### Step 3: Sum the results
Adding the results from the three integrals:
\[
18 + 0 + 0 = 18
\]

### Step 4: Numerical approximation
The exact answer is 18, so the numerical approximation is:
\[
18.0000000000
\]

### Final Answer
```json
{"answer": "18", "numerical_answer": "18.0000000000"}
```