

To calculate the definite integral \(\int_1^2 \left(2^{x-1} + \log_2(2x)\right) \, dx\), we split it into two separate integrals and evaluate each part analytically.

### Step 1: Evaluate \(\int_1^2 2^{x-1} \, dx\)
The integral of \(2^{x-1}\) with respect to \(x\) is found using the formula for integrating exponential functions:  
\[
\int a^u \, du = \frac{a^u}{\ln(a)} + C \quad (a > 0, a \neq 1)
\]  
Let \(u = x - 1\), so \(du = dx\). Then:  
\[
\int 2^{x-1} \, dx = \frac{2^{x-1}}{\ln(2)} + C
\]  
Evaluating from \(1\) to \(2\):  
\[
\left. \frac{2^{x-1}}{\ln(2)} \right|_1^2 = \frac{2^{2-1}}{\ln(2)} - \frac{2^{1-1}}{\ln(2)} = \frac{2}{\ln(2)} - \frac{1}{\ln(2)} = \frac{1}{\ln(2)}
\]

### Step 2: Evaluate \(\int_1^2 \log_2(2x) \, dx\)
First, simplify \(\log_2(2x)\) using logarithm properties:  
\[
\log_2(2x) = \log_2(2) + \log_2(x) = 1 + \log_2(x)
\]  
Thus, the integral becomes:  
\[
\int_1^2 \left(1 + \log_2(x)\right) \, dx = \int_1^2 1 \, dx + \int_1^2 \log_2(x) \, dx
\]  

- The first term \(\int_1^2 1 \, dx\) is straightforward:  
  \[
  \int_1^2 1 \, dx = \left. x \right|_1^2 = 2 - 1 = 1
  \]  

- For the second term \(\int_1^2 \log_2(x) \, dx\), convert to natural logarithm:  
  \[
  \log_2(x) = \frac{\ln(x)}{\ln(2)}
  \]  
  The integral of \(\ln(x)\) is \(x \ln(x) - x + C\), so:  
  \[
  \int \log_2(x) \, dx = \frac{1}{\ln(2)} \int \ln(x) \, dx = \frac{1}{\ln(2)} \left( x \ln(x) - x \right) + C
  \]  
  Evaluating from \(1\) to \(2\):  
  \[
  \left. \frac{1}{\ln(2)} \left( x \ln(x) - x \right) \right|_1^2 = \frac{1}{\ln(2)} \left[ (2 \ln(2) - 2) - (1 \ln(1) - 1) \right]
  \]  
  Since \(\ln(1) = 0\), this simplifies to:  
  \[
  \frac{1}{\ln(2)} \left[ (2 \ln(2) - 2) - (-1) \right] = \frac{1}{\ln(2)} \left( 2 \ln(2) - 1 \right) = 2 - \frac{1}{\ln(2)}
  \]  

Combining the two terms:  
\[
\int_1^2 \log_2(2x) \, dx = 1 + \left( 2 - \frac{1}{\ln(2)} \right) = 3 - \frac{1}{\ln(2)}
\]

### Step 3: Combine the results
Adding the two integrals:  
\[
\int_1^2 \left(2^{x-1} + \log_2(2x)\right) \, dx = \frac{1}{\ln(2)} + \left( 3 - \frac{1}{\ln(2)} \right) = 3
\]

### Numerical Approximation
The exact result is \(3\), so the numerical approximation (rounded to 10 decimal places) is \(3.0000000000\).

{"answer": "3", "numerical_answer": "3.0000000000"}