To solve the definite integral 

\[
\int_{64}^{729} \frac{x^{1/2}}{x^{1/2} - x^{1/3} \, dx,
\]

we first simplify the integrand:

\[
\frac{x^{1/2}}{x^{1/2} - x^{1/3}} = \frac{x^{1/2}}{x^{1/2} - x^{1/3}}.
\]

### Step 1: Simplify the Integrand
Factor out \( x^{1/3} \) from the denominator:

\[
x^{1/2} - x^{1/3} = x^{1/3} (x^{1/6} - 1).
\]

Thus, the integrand becomes:

\[
\frac{x^{1/2}}{x^{1/3} (x^{1/6} - 1)} = \frac{x^{1/6}}{x^{1/6} - 1}.
\]

### Step 2: Perform a Substitution
Let \( u = x^{1/6} \). Then:

\[
du = \frac{1}{6} x^{-5/6} dx \implies dx = 6 x^{5/6} du = 6 u^5 du.
\]

Change the limits:
- When \( x = 64 \), \( u = 64^{1/6} = 2 \).
- When \( x = 729 \), \( u = 729^{1/6} = 3 \).

Substitute into the integral:

\[
\int_{2}^{3} \frac{u}{u - 1} \cdot 6 u^5 du = 6 \int_{2}^{3} \frac{u^6}{u - 1} du.
\]

### Step 3: Simplify the New Integrand
Perform polynomial long division on \( \frac{u^6}{u - 1} \):

\[
\frac{u^6}{u - 1} = u^5 + u^4 + u^3 + u^2 + u + 1 + \frac{1}{u - 1}.
\]

Thus, the integral becomes:

\[
6 \int_{2}^{3} \left( u^5 + u^4 + u^3 + u^2 + u + 1 + \frac{1}{u - 1} \right) du.
\]

### Step 4: Integrate Term by Term
Integrate each term separately:

\[
6 \left[ \frac{u^6}{6} + \frac{u^5}{5} + \frac{u^4}{4} + \frac{u^3}{3} + \frac{u^2}{2} + u + \ln|u - 1| \right]_{2}^{3}.
\]

Evaluate at the bounds:

At \( u = 3 \):

\[
\frac{3^6}{6} + \frac{3^5}{5} + \frac{3^4}{4} + \frac{3^3}{3} + \frac{3^2}{2} + 3 + \ln 2 = \frac{729}{6} + \frac{243}{5} + \frac{81}{4} + 9 + \frac{9}{2} + 3 + \ln 2.
\]

At \( u = 2 \):

\[
\frac{2^6}{6} + \frac{2^5}{5} + \frac{2^4}{4} + \frac{2^3}{3} + \frac{2^2}{2} + 2 + \ln 1 = \frac{64}{6} + \frac{32}{5} + \frac{16}{4} + \frac{8}{3} + \frac{4}{2} + 2 + 0.
\]

Compute the difference:

\[
6 \left( \left( \frac{729}{6} + \frac{243}{5} + \frac{81}{4} + 9 + \frac{9}{2} + 3 + \ln 2 \right) - \left( \frac{64}{6} + \frac{32}{5} + \frac{16}{4} + \frac{8}{3} + \frac{4}{2} + 2 \right) \right).
\]

Simplify the constants:

\[
6 \left( \frac{729 - 64}{6} + \frac{243 - 32}{5} + \frac{81 - 16}{4} + \left(9 - \frac{8}{3}\right) + \left(\frac{9}{2} - \frac{4}{2}\right) + (3 - 2) + \ln 2 \right).
\]

\[
6 \left( \frac{665}{6} + \frac{211}{5} + \frac{65}{4} + \frac{19}{3} + \frac{5}{2} + 1 + \ln 2 \right).
\]

Combine the terms:

\[
6 \left( \frac{665}{6} + \frac{211}{5} + \frac{65}{4} + \frac{19}{3} + \frac{5}{2} + 1 + \ln 2 \right).
\]

Compute the numerical value:

\[
\frac{665}{6} \approx 110.8333, \quad \frac{211}{5} = 42.2, \quad \frac{65}{4} = 16.25, \quad \frac{19}{3} \approx 6.3333, \quad \frac{5}{2} = 2.5, \quad 1 = 1.
\]

Sum:

\[
110.8333 + 42.2 + 16.25 + 6.3333 + 2.5 + 1 + \ln 2 \approx 179.1166 + 0.6931 = 179.8097.
\]

Multiply by 6:

\[
6 \times 179.8097 \approx 1078.8582.
\]

### Step 5: Numerical Approximation
The numerical approximation of the integral is approximately \( 1078.8582116407 \).

### Final Answer
\[
\boxed{
{"answer": "6 \left( \frac{665}{6} + \frac{211}{5} + \frac{65}{4} + \frac{19}{3} + \frac{5}{2} + 1 + \ln 2 \right)", "numerical_answer": "1078.8582116407"}
}
\]