# Evaluating $\int_0^{\pi/2}\frac{\cos(x)}{2-\cos^2(x)}dx$

## Step 1: Substitution
Let's make a substitution to simplify this integral. Let $u = \cos(x)$, then $du = -\sin(x)dx$, which gives $dx = -\frac{du}{\sin(x)}$.

When $x = 0$, $u = \cos(0) = 1$
When $x = \pi/2$, $u = \cos(\pi/2) = 0$

We also need to express $\sin(x)$ in terms of $u$. Since $\cos^2(x) + \sin^2(x) = 1$, we have $\sin(x) = \sqrt{1-\cos^2(x)} = \sqrt{1-u^2}$.

So $dx = -\frac{du}{\sqrt{1-u^2}}$.

The integral becomes:
$$\int_0^{\pi/2}\frac{\cos(x)}{2-\cos^2(x)}dx = \int_1^0 \frac{u}{2-u^2} \cdot \left(-\frac{1}{\sqrt{1-u^2}}\right) du$$

Adjusting the limits and sign:
$$\int_0^{\pi/2}\frac{\cos(x)}{2-\cos^2(x)}dx = \int_1^0 \frac{-u}{(2-u^2)\sqrt{1-u^2}} du = \int_0^1 \frac{u}{(2-u^2)\sqrt{1-u^2}} du$$

## Step 2: Algebraic manipulation
Let's analyze the integrand $\frac{u}{(2-u^2)\sqrt{1-u^2}}$. 

We can rewrite $2-u^2 = 2(1-\frac{u^2}{2})$ and factor the denominator:
$$\frac{u}{(2-u^2)\sqrt{1-u^2}} = \frac{u}{2(1-\frac{u^2}{2})\sqrt{1-u^2}} = \frac{u}{2\sqrt{1-u^2}(1-\frac{u^2}{2})}$$

## Step 3: Further substitution
Let's try another substitution: $v = u^2$, which gives $dv = 2u\,du$ or $du = \frac{dv}{2u}$.

When $u = 0$, $v = 0$
When $u = 1$, $v = 1$

The integral becomes:
$$\int_0^1 \frac{u}{(2-u^2)\sqrt{1-u^2}} du = \int_0^1 \frac{u}{2\sqrt{1-u^2}(1-\frac{u^2}{2})} du$$

$$= \int_0^1 \frac{1}{2\sqrt{1-u^2}(1-\frac{u^2}{2})} \cdot \frac{dv}{2} = \int_0^1 \frac{1}{4\sqrt{1-v}(1-\frac{v}{2})} dv$$

## Step 4: Partial fractions
Let's use partial fractions on $\frac{1}{4(1-\frac{v}{2})}$:

$$\frac{1}{4(1-\frac{v}{2})} = \frac{1}{4(1-\frac{v}{2})} = \frac{1}{4\cdot\frac{2-v}{2}} = \frac{1}{2(2-v)}$$

So our integral is:
$$\int_0^1 \frac{1}{2(2-v)\sqrt{1-v}} dv$$

## Step 5: Another substitution
Let $w = 1-v$, which gives $dv = -dw$. 
When $v = 0$, $w = 1$
When $v = 1$, $w = 0$

The integral becomes:
$$\int_0^1 \frac{1}{2(2-v)\sqrt{1-v}} dv = \int_1^0 \frac{1}{2(2-(1-w))\sqrt{w}} (-dw) = \int_0^1 \frac{1}{2(1+w)\sqrt{w}} dw$$

## Step 6: Standard form
We recognize this as a standard form:
$$\int_0^1 \frac{1}{2(1+w)\sqrt{w}} dw = \frac{1}{2}\int_0^1 \frac{1}{(1+w)\sqrt{w}} dw$$

This is related to the arctangent function. We can solve it by using the substitution $t = \sqrt{w}$, which gives $w = t^2$ and $dw = 2t\,dt$.

When $w = 0$, $t = 0$
When $w = 1$, $t = 1$

$$\frac{1}{2}\int_0^1 \frac{1}{(1+w)\sqrt{w}} dw = \frac{1}{2}\int_0^1 \frac{1}{(1+t^2)t} \cdot 2t\,dt = \int_0^1 \frac{1}{1+t^2} dt = \arctan(t)\Big|_0^1$$

$$= \arctan(1) - \arctan(0) = \frac{\pi}{4} - 0 = \frac{\pi}{4}$$

## Step 7: Numerical approximation
The exact value is $\frac{\pi}{4}$, which numerically equals $0.7853981634$ (rounded to 10 decimal places).

Therefore, the definite integral $\int_0^{\pi/2}\frac{\cos(x)}{2-\cos^2(x)}dx = \frac{\pi}{4} \approx 0.7853981634$.

{"answer": "\\frac{\\pi}{4}", "numerical_answer": "0.7853981634"}