Let's proceed step by step.

**Step 1: Analytical computation of the integral**
\[
I = \int_0^\infty \frac{x}{e^x - 1}\, dx
\]

Recall that:
\[
\frac{1}{e^x - 1} = \sum_{n=1}^\infty e^{-nx}, \quad \text{for } x > 0
\]

So,
\[
I = \int_0^\infty x \left( \sum_{n=1}^\infty e^{-nx} \right) dx = \sum_{n=1}^\infty \int_0^\infty x e^{-nx} dx
\]

Letâ€™s compute the inner integral:
\[
\int_0^\infty x e^{-n x} dx
\]

Let \( u = x \), \( dv = e^{-n x} dx \Rightarrow v = -\frac{1}{n}e^{-n x} \):

Integration by parts:
\[
\int x e^{-n x} dx = -\frac{x}{n}e^{-n x} + \frac{1}{n}\int e^{-n x} dx
= -\frac{x}{n}e^{-n x} - \frac{1}{n^2}e^{-n x} + C
\]

Evaluate from \( 0 \) to \( \infty \):

At \( x \to \infty \), \( x e^{-n x} \to 0 \), \( e^{-n x} \to 0 \).
At \( x = 0 \):
\[
-\frac{0}{n}e^{0} - \frac{1}{n^2}e^{0} = -\frac{1}{n^2}
\]

So,
\[
\int_0^\infty x e^{-n x} dx = 0 - \left(-\frac{1}{n^2}\right) = \frac{1}{n^2}
\]

Continue with sum:
\[
I = \sum_{n=1}^\infty \frac{1}{n^2}
\]

But this is the definition of the Riemann zeta function at \( s=2 \):

\[
\zeta(2) = \sum_{n=1}^\infty \frac{1}{n^2}
\]

And it's well known:
\[
\zeta(2) = \frac{\pi^2}{6}
\]

**Step 2: All steps are shown above.**

**Step 3: Numerical evaluation**

\[
\frac{\pi^2}{6} \approx 1.6449340668
\]

**Step 4: JSON output**

```json
{"answer": "\\frac{\\pi^2}{6}", "numerical_answer": "1.6449340668"}
```