<think>
Okay, let's tackle this integral step by step. The integral given is ∫ from -3/2 to -1/2 of (x⁵ + 5x⁴ + 10x³ + 8x² + x) dx. Hmm, first, I need to compute the antiderivative of each term separately. 

Starting with x⁵. The integral of x^n is (x^(n+1))/(n+1), so for x⁵, that would be (x⁶)/6. Next term is 5x⁴. The integral of 5x⁴ is 5*(x⁵)/5, which simplifies to x⁵. Then, 10x³. Integrating that gives 10*(x⁴)/4, which is (10/4)x⁴ or (5/2)x⁴. Wait, maybe I should keep it as fractions to avoid decimal confusion. So 10/4 reduces to 5/2, right.

Next term is 8x². The integral is 8*(x³)/3, so (8/3)x³. Then the term x. The integral of x is (x²)/2. So putting all these together, the antiderivative F(x) should be:

F(x) = (1/6)x⁶ + x⁵ + (5/2)x⁴ + (8/3)x³ + (1/2)x²

Now, I need to evaluate this from -3/2 to -1/2. So compute F(-1/2) - F(-3/2). Let's compute each part step by step.

First, let's compute F(-1/2):

Calculate each term:

1. (1/6)(-1/2)^6: (-1/2)^6 is (1/2)^6 = 1/64. So (1/6)*(1/64) = 1/384 ≈ 0.0026041667

2. (-1/2)^5: (-1/2)^5 = -1/32. So this term is -1/32 ≈ -0.03125

3. (5/2)*(-1/2)^4: (-1/2)^4 = 1/16. Multiply by 5/2: (5/2)*(1/16) = 5/32 ≈ 0.15625

4. (8/3)*(-1/2)^3: (-1/2)^3 = -1/8. Multiply by 8/3: (8/3)*(-1/8) = -1/3 ≈ -0.3333333333

5. (1/2)*(-1/2)^2: (-1/2)^2 = 1/4. Multiply by 1/2: 1/8 = 0.125

Adding these up:

1/384 -1/32 +5/32 -1/3 +1/8

Let me convert all to 384 denominator to add:

1/384 - 12/384 + 60/384 -128/384 +48/384

Adding numerators: 1 -12 +60 -128 +48 = (1-12) = -11; (-11 +60)=49; (49-128)= -79; (-79+48)= -31. So total is -31/384 ≈ -0.0807291667

Now compute F(-3/2):

Each term:

1. (1/6)*(-3/2)^6: (-3/2)^6 = (3/2)^6 = (729)/(64). So (1/6)*(729/64) = 729/384 = 243/128 ≈ 1.8984375

2. (-3/2)^5: (-3/2)^5 = -243/32. So this term is -243/32 ≈ -7.59375

3. (5/2)*(-3/2)^4: (-3/2)^4 = 81/16. Multiply by 5/2: (5/2)*(81/16) = 405/32 ≈ 12.65625

4. (8/3)*(-3/2)^3: (-3/2)^3 = -27/8. Multiply by 8/3: (8/3)*(-27/8) = -9 ≈ -9.0

5. (1/2)*(-3/2)^2: (-3/2)^2 = 9/4. Multiply by 1/2: 9/8 ≈ 1.125

Now add all these terms:

243/128 -243/32 +405/32 -9 +9/8

Convert all to 128 denominator:

243/128 - (243/32)*(4/4) = -243*4/128 = -972/128

Similarly, 405/32 = 405*4/128 = 1620/128

-9 is -9*128/128 = -1152/128

9/8 = 144/128

So total:

243 -972 +1620 -1152 +144 all over 128

Calculate numerator:

243 -972 = -729

-729 +1620 = 891

891 -1152 = -261

-261 +144 = -117

So total is -117/128 ≈ -0.9140625

So F(-3/2) is -117/128 ≈ -0.9140625

Wait, but wait, let me check again. Wait, when I converted each term:

First term: 243/128

Second term: -243/32 = -972/128

Third term: 405/32 = 1620/128

Fourth term: -9 = -1152/128

Fifth term: 9/8 = 144/128

So adding all numerators:

243 -972 +1620 -1152 +144

Let me compute step by step:

243 -972 = -729

-729 +1620 = 891

891 -1152 = -261

-261 +144 = -117

Yes, so total is -117/128. So F(-3/2) = -117/128 ≈ -0.9140625

Now, the definite integral is F(-1/2) - F(-3/2) = (-31/384) - (-117/128) = (-31/384) + 117/128

Convert 117/128 to 384 denominator: 117/128 = (117*3)/(128*3) = 351/384

So total is (-31 + 351)/384 = 320/384 = 320 ÷ 32 = 10; 384 ÷32=12. So 10/12 = 5/6 ≈0.8333333333

Wait, 320/384 simplifies by dividing numerator and denominator by 64: 320 ÷64=5, 384 ÷64=6. So 5/6. So exact value is 5/6. The numerical approximation is approximately 0.8333333333.

Wait, but let me check again. Because when I computed F(-1/2) as -31/384 and F(-3/2) as -117/128. Then F(-1/2) - F(-3/2) is (-31/384) - (-117/128) = (-31/384) + 117/128. Let's compute 117/128 as 351/384. So 351 -31 = 320. 320/384 = 5/6. Yes, that's correct.

So the exact answer is 5/6, and the numerical approximation is approximately 0.8333333333. Rounded to 10 decimal places, that's 0.8333333333.

But wait, maybe I made a mistake in the calculation. Let me verify again.

Alternatively, maybe there's a smarter way to check. Let's see, the integrand is x⁵ +5x⁴ +10x³ +8x² +x. Hmm, perhaps this polynomial can be factored or simplified. Let me check if it's a derivative of some product. Let me see.

Let me consider (x +1)^5. Expanding that:

(x+1)^5 = x^5 +5x^4 +10x³ +10x² +5x +1. Hmm, but our integrand is x^5 +5x^4 +10x³ +8x² +x. So the difference is in the x² and x terms. The given polynomial is (x+1)^5 - 2x² -4x -1. Wait, maybe not. Let me check:

(x+1)^5 = x^5 +5x^4 +10x³ +10x² +5x +1. So if we subtract 2x² +4x +1, we get x^5 +5x^4 +10x³ +8x² +x. Which matches the integrand. So the integrand is (x+1)^5 -2x² -4x -1. Hmm, maybe that's easier to integrate.

But perhaps integrating term by term is straightforward. But maybe this approach can help check. Let's see:

Integral of (x+1)^5 is (x+1)^6 /6. Then integral of -2x² is -2*(x³)/3, integral of -4x is -4*(x²)/2 = -2x², integral of -1 is -x. So the antiderivative would be (x+1)^6/6 - (2/3)x³ -2x² -x. Then evaluate from -3/2 to -1/2.

But maybe this approach is more complicated. Alternatively, let's check if the previous result of 5/6 is correct. Let's compute using this alternative method.

Compute F(-1/2) using the new antiderivative:

(x+1)^6 /6 evaluated at x=-1/2: ( (-1/2 +1) )^6 /6 = (1/2)^6 /6 = (1/64)/6 = 1/384 ≈0.0026041667

Then subtract (2/3)x³: (2/3)*(-1/2)^3 = (2/3)*(-1/8) = -1/12 ≈-0.0833333333

Subtract 2x²: 2*(-1/2)^2 = 2*(1/4) = 1/2 =0.5

Subtract x: -(-1/2) = 1/2 =0.5

So total F(-1/2) = 1/384 - (-1/12) -0.5 -0.5? Wait, no. Wait, the antiderivative is (x+1)^6/6 - (2/3)x³ -2x² -x. So when evaluating at x=-1/2:

= (1/2)^6 /6 - (2/3)*(-1/2)^3 -2*(-1/2)^2 - (-1/2)

= 1/(64*6) - (2/3)*(-1/8) -2*(1/4) +1/2

= 1/384 + (1/12) - 0.5 +0.5

Wait, 1/384 +1/12. 1/12 is 32/384. So 1+32=33/384 = 11/128 ≈0.0859375. Then -0.5 +0.5 cancels. So F(-1/2) =11/128 ≈0.0859375. Wait, but this contradicts the previous result where F(-1/2) was -31/384 ≈-0.0807291667. So there's a mistake here. Therefore, my alternative approach must be wrong. So perhaps the integrand isn't exactly (x+1)^5 -2x² -4x -1. Let me check again.

Original integrand: x⁵ +5x⁴ +10x³ +8x² +x.

(x+1)^5 is x⁵ +5x⁴ +10x³ +10x² +5x +1. So subtract 2x² +4x +1 to get x⁵ +5x⁴ +10x³ +8x² +x. So yes, integrand is (x+1)^5 -2x² -4x -1. Therefore, the antiderivative should be (x+1)^6 /6 - (2/3)x³ -2x² -x + C. But when I evaluated this at x=-1/2, I get:

(x+1)^6 /6 = (1/2)^6 /6 =1/384 ≈0.0026041667

Then - (2/3)x³: x=-1/2, so x³=-1/8. So - (2/3)*(-1/8)= 1/12 ≈0.0833333333

-2x²: x=-1/2, x²=1/4. So -2*(1/4)= -0.5

- x: -(-1/2)=0.5

So total: 1/384 +1/12 -0.5 +0.5 =1/384 +1/12. 1/12 is 32/384, so 33/384=11/128≈0.0859375. But earlier calculation using term-by-term integration gave F(-1/2)= -31/384≈-0.0807291667. There's a discrepancy here. So I must have made a mistake in one of the methods.

Wait, this suggests that my initial term-by-term integration was wrong. Let me check that again.

Original antiderivative term-by-term:

(1/6)x⁶ +x⁵ + (5/2)x⁴ + (8/3)x³ + (1/2)x².

Evaluated at x=-1/2:

(1/6)(-1/2)^6 + (-1/2)^5 + (5/2)(-1/2)^4 + (8/3)(-1/2)^3 + (1/2)(-1/2)^2.

Compute each term:

1. (1/6)(1/64) =1/384 ≈0.0026041667

2. (-1/32)≈-0.03125

3. (5/2)(1/16)=5/32≈0.15625

4. (8/3)(-1/8)= -1/3≈-0.3333333333

5. (1/2)(1/4)=1/8=0.125

Adding these:

0.0026041667 -0.03125 +0.15625 -0.3333333333 +0.125

Let's compute step by step:

0.0026041667 -0.03125 = -0.0286458333

-0.0286458333 +0.15625 =0.1276041667

0.1276041667 -0.3333333333 = -0.2057291666

-0.2057291666 +0.125 = -0.0807291666 ≈-0.0807291666, which is -31/384. Because 31*0.0026041667≈0.0807291667. So 31/384≈0.0807291667, so negative of that is -0.0807291667.

But according to the other method, using the factored integrand, the result is 11/128≈0.0859375. These two results should be the same, but they are not. Therefore, there's a mistake in one of the methods.

Wait, this means that either the term-by-term integration is wrong, or the alternative approach is wrong. Let me check the alternative approach again.

The integrand is (x+1)^5 -2x² -4x -1. Therefore, the antiderivative should be (x+1)^6/6 - (2/3)x³ -2x² -x + C. Let's compute this at x=-1/2:

(x+1)^6/6 = ( (-1/2 +1) )^6 /6 = (1/2)^6 /6 =1/64 /6=1/384≈0.0026041667

Then, - (2/3)x³: x=-1/2, x³= -1/8. So - (2/3)*(-1/8)=1/12≈0.0833333333

-2x²: x=-1/2, x²=1/4. So -2*(1/4)= -0.5

- x: -(-1/2)=0.5

Adding these: 0.0026041667 +0.0833333333 -0.5 +0.5 =0.0026041667 +0.0833333333=0.0859375. Which is 11/128≈0.0859375. But according to term-by-term integration, it's -31/384≈-0.0807291667. These are different. Therefore, there's a mistake in one of the antiderivatives.

Wait, but the integrand is x⁵ +5x⁴ +10x³ +8x² +x. Let's compute (x+1)^5 -2x² -4x -1:

(x+1)^5 =x^5 +5x^4 +10x^3 +10x^2 +5x +1

Subtract 2x² +4x +1: gives x^5 +5x^4 +10x^3 +8x² +x. Correct. So the integrand is correct. Therefore, the antiderivative via this method should be correct. Therefore, the term-by-term integration must have an error.

Let me check the term-by-term antiderivative again. The integral of x⁵ is (1/6)x^6. Correct. Integral of 5x⁴ is x^5. Correct. Integral of 10x³ is 10*(x^4)/4= (5/2)x^4. Correct. Integral of 8x² is 8*(x^3)/3. Correct. Integral of x is (1/2)x². Correct. So the antiderivative is correct. Therefore, why the discrepancy?

Wait, when evaluating F(-1/2) using term-by-term, I get -31/384≈-0.0807291667, but using the other method, I get 11/128≈0.0859375. These should be the same. Therefore, there's a mistake in one of the evaluations.

Let me re-calculate F(-1/2) using the term-by-term antiderivative:

F(x) = (1/6)x⁶ +x⁵ + (5/2)x⁴ + (8/3)x³ + (1/2)x²

At x=-1/2:

Compute each term:

1. (1/6)(-1/2)^6 = (1/6)(1/64) =1/384 ≈0.0026041667

2. (-1/2)^5 = -1/32 ≈-0.03125

3. (5/2)(-1/2)^4 = (5/2)(1/16)=5/32≈0.15625

4. (8/3)(-1/2)^3 = (8/3)(-1/8)= -1/3≈-0.3333333333

5. (1/2)(-1/2)^2 = (1/2)(1/4)=1/8=0.125

Now sum them up:

0.0026041667 -0.03125 +0.15625 -0.3333333333 +0.125

Let's compute step by step:

Start with 0.0026041667

Subtract 0.03125: 0.0026041667 -0.03125 = -0.0286458333

Add 0.15625: -0.0286458333 +0.15625 =0.1276041667

Subtract 0.3333333333: 0.1276041667 -0.3333333333 = -0.2057291666

Add 0.125: -0.2057291666 +0.125 = -0.0807291666 ≈-0.0807291666

Which is -31/384. But according to the other method, it's 11/128≈0.0859375. So there's a discrepancy. Therefore, one of the antiderivatives is wrong. But both methods should give the same result. Let me check the antiderivative from the factored integrand.

The antiderivative via factoring is (x+1)^6/6 - (2/3)x³ -2x² -x + C. Let's expand this to see if it matches the term-by-term antiderivative.

Expand (x+1)^6:

(x+1)^6 = x^6 +6x^5 +15x^4 +20x^3 +15x^2 +6x +1

So (x+1)^6/6 = (1/6)x^6 +x^5 + (15/6)x^4 + (20/6)x^3 + (15/6)x^2 + (6/6)x +1/6

Simplify:

= (1/6)x^6 +x^5 + (5/2)x^4 + (10/3)x^3 + (5/2)x^2 +x +1/6

Now subtract (2/3)x³ -2x² -x:

So the antiderivative is:

(1/6)x^6 +x^5 + (5/2)x^4 + (10/3)x^3 + (5/2)x^2 +x +1/6 - (2/3)x³ -2x² -x

Combine like terms:

x^6/6 +x^5 +5x^4/2 + (10/3 -2/3)x³ + (5/2 -2)x² + (x -x) +1/6

Simplify:

x^6/6 +x^5 +5x^4/2 +8x³/3 + (5/2 -4/2)x² +0 +1/6

Which is:

x^6/6 +x^5 +5x^4/2 +8x³/3 + (1/2)x² +1/6

But the term-by-term antiderivative was:

(1/6)x^6 +x^5 + (5/2)x^4 + (8/3)x³ + (1/2)x²

Comparing the two, the factored method's antiderivative has an extra +1/6. Therefore, the correct antiderivative via factoring should be:

(x+1)^6/6 - (2/3)x³ -2x² -x + C. But when expanded, it's the term-by-term antiderivative plus 1/6. Therefore, there's a constant difference. So when evaluating the definite integral, the constants will cancel out. Therefore, when we compute F(b) - F(a), the constants will subtract, so the 1/6 cancels. Therefore, both methods should give the same result. But in our case, when we computed F(-1/2) using the term-by-term method, we didn't include the +1/6, but the factored method does. Wait, but in the term-by-term integration, we didn't have the +1/6. Therefore, the antiderivatives differ by a constant, which is 1/6. Therefore, when we compute F(-1/2) - F(-3/2), the constants will cancel. Let's check.

Using the factored antiderivative:

F(-1/2) = (1/2)^6/6 - (2/3)(-1/2)^3 -2*(-1/2)^2 - (-1/2) +1/6

Wait, no. Wait, the antiderivative from factoring is (x+1)^6/6 - (2/3)x³ -2x² -x. There's no +1/6. Wait, when expanding (x+1)^6/6, we get the term-by-term antiderivative plus 1/6. So the antiderivative via factoring is the term-by-term antiderivative plus 1/6. Therefore, when we compute F(b) - F(a), the 1/6 cancels out. Therefore, the definite integral should be the same. Therefore, the term-by-term result was -31/384 - (-117/128) =5/6, and the factored method would give the same. Let's compute using the factored antiderivative.

Compute F(-1/2) - F(-3/2) using factored antiderivative:

F(-1/2) = (1/2)^6/6 - (2/3)(-1/2)^3 -2*(-1/2)^2 - (-1/2)

= (1/64)/6 - (2/3)(-1/8) -2*(1/4) +1/2

= 1/384 +1/12 -0.5 +0.5

=1/384 +1/12 = (1 +32)/384 =33/384=11/128≈0.0859375

F(-3/2) = ( (-3/2 +1)^6 )/6 - (2/3)(-3/2)^3 -2*(-3/2)^2 - (-3/2)

First, (-3/2 +1) = (-1/2). So (-1/2)^6=1/64. So (1/64)/6=1/384≈0.0026041667

Next term: - (2/3)*(-3/2)^3 = - (2/3)*(-27/8)= (54/24)=9/4=2.25

Wait, let's compute each term:

1. ( (-3/2 +1)^6 )/6 = (-1/2)^6 /6 =1/64 /6=1/384≈0.0026041667

2. - (2/3)*(-3/2)^3: (-3/2)^3= -27/8. So - (2/3)*(-27/8)= (54/24)=9/4=2.25

3. -2*(-3/2)^2: (-3/2)^2=9/4. So -2*(9/4)= -9/2= -4.5

4. - (-3/2)=1.5

So F(-3/2)=1/384 +9/4 -9/2 +3/2

Convert all to 384 denominator:

1/384 + (9/4)*(96/96)= 864/384

-9/2= -1728/384

3/2=576/384

So total:

1 +864 -1728 +576 all over 384

Numerator:1 +864=865; 865 -1728= -863; -863 +576= -287

Wait, that can't be right. Wait, 9/4 is 216/96, but maybe better to compute step by step:

1/384 +9/4 =1/384 + 864/384=865/384

Then subtract 9/2: 865/384 - 1728/384= (865-1728)/384= -863/384

Then add 3/2: -863/384 + 576/384= (-863 +576)/384= -287/384≈-0.7473958333

But according to term-by-term, F(-3/2) was -117/128≈-0.9140625. So there's a problem here. Therefore, there's a mistake in the calculation using the factored antiderivative. Let me recheck.

Wait, step 2: - (2/3)*(-3/2)^3. Let's compute (-3/2)^3= -27/8. So - (2/3)*(-27/8)= (2*27)/(3*8)=54/24=9/4=2.25. Correct.

Step 3: -2*(-3/2)^2. (-3/2)^2=9/4. So -2*(9/4)= -9/2= -4.5. Correct.

Step 4: - (-3/2)=3/2=1.5. Correct.

So F(-3/2)=1/384 +9/4 -9/2 +3/2

Compute step by step:

1/384 ≈0.0026041667

+9/4=2.25 → 0.0026041667 +2.25=2.2526041667

-9/2= -4.5 →2.2526041667 -4.5= -2.2473958333

+3/2=1.5 →-2.2473958333 +1.5= -0.7473958333≈-0.7473958333

But according to term-by-term, F(-3/2)= -117/128≈-0.9140625. So there's a discrepancy. Therefore, the two methods are not equivalent, which suggests that there's a mistake in one of the antiderivatives. But we know that the integrand is correctly expressed as (x+1)^5 -2x² -4x -1, so the antiderivative should be correct. Therefore, the term-by-term integration must have an error. But when we expanded the factored antiderivative, it was equal to the term-by-term antiderivative plus 1/6. Therefore, the term-by-term antiderivative is missing the 1/6 from the expansion. Therefore, the correct antiderivative should include that 1/6. But in the term-by-term integration, we didn't include it. Therefore, the mistake is in the term-by-term integration. Wait, no. The term-by-term integration integrates each term of the original polynomial, which is x⁵ +5x⁴ +10x³ +8x² +x. The antiderivative of that is (1/6)x⁶ +x⁵ + (10/4)x⁴ + (8/3)x³ + (1/2)x². Which is correct. The expansion of the factored antiderivative gives the same terms plus 1/6. Therefore, the two antiderivatives differ by a constant 1/6. Therefore, when computing the definite integral, the constants cancel. Therefore, F(b) - F(a) should be the same in both methods. Let's check:

Using the term-by-term method, F(-1/2) - F(-3/2) = (-31/384) - (-117/128) =5/6≈0.8333333333.

Using the factored method, F(-1/2) - F(-3/2) = (11/128) - (-287/384). Let's compute this:

11/128 = 33/384

So 33/384 - (-287/384) = (33 +287)/384=320/384=5/6. So yes, the definite integral is 5/6. Therefore, the discrepancy in the antiderivatives is due to the constant difference, which cancels out in definite integrals. Therefore, the correct answer is 5/6. Therefore, the initial calculation was correct. The numerical approximation is 0.8333333333.

So the final answer is {"answer": "\\dfrac{5}{6}", "numerical_answer": "0.8333333333"}
</think>

{"answer": "\\dfrac{5}{6}", "numerical_answer": "0.8333333333"}