# Evaluating $\int\limits_{0}^{\infty}\frac{x^{2}}{e^x-1}\left[2^{3}\sinh\left(0.5x\right)-\sinh\left(0.25x\right)\right]dx$

## Step 1: Rewrite the integrand
First, recall that $\sinh(ax) = \frac{e^{ax} - e^{-ax}}{2}$. Let's substitute this:

$2^3\sinh(0.5x) - \sinh(0.25x) = 8\cdot\frac{e^{0.5x} - e^{-0.5x}}{2} - \frac{e^{0.25x} - e^{-0.25x}}{2}$

$= 4(e^{0.5x} - e^{-0.5x}) - \frac{1}{2}(e^{0.25x} - e^{-0.25x})$

$= 4e^{0.5x} - 4e^{-0.5x} - \frac{1}{2}e^{0.25x} + \frac{1}{2}e^{-0.25x}$

## Step 2: Use the Riemann zeta function
For the integral $\int_0^{\infty} \frac{x^n e^{-ax}}{1-e^{-x}}dx$, we can use the formula:
$\int_0^{\infty} \frac{x^n e^{-ax}}{1-e^{-x}}dx = n! \zeta(n+1, a)$

Where $\zeta(s, a)$ is the Hurwitz zeta function. When $a=1$, we get the Riemann zeta function.

We can rewrite our integral by multiplying both numerator and denominator by $e^{-x}$:
$\int\limits_{0}^{\infty}\frac{x^{2}}{e^x-1}\left[2^{3}\sinh\left(0.5x\right)-\sinh\left(0.25x\right)\right]dx = \int\limits_{0}^{\infty}\frac{x^{2}e^{-x}}{1-e^{-x}}\left[2^{3}\sinh\left(0.5x\right)-\sinh\left(0.25x\right)\right]dx$

## Step 3: Substitute the expression for the sinh terms
Using our decomposition from Step 1:

$\int\limits_{0}^{\infty}\frac{x^{2}e^{-x}}{1-e^{-x}}\left[4e^{0.5x} - 4e^{-0.5x} - \frac{1}{2}e^{0.25x} + \frac{1}{2}e^{-0.25x}\right]dx$

This gives us:
$\int\limits_{0}^{\infty}\frac{x^{2}e^{-x}}{1-e^{-x}}4e^{0.5x}dx - \int\limits_{0}^{\infty}\frac{x^{2}e^{-x}}{1-e^{-x}}4e^{-0.5x}dx - \int\limits_{0}^{\infty}\frac{x^{2}e^{-x}}{1-e^{-x}}\frac{1}{2}e^{0.25x}dx + \int\limits_{0}^{\infty}\frac{x^{2}e^{-x}}{1-e^{-x}}\frac{1}{2}e^{-0.25x}dx$

Simplifying the exponents:
$4\int\limits_{0}^{\infty}\frac{x^{2}e^{-0.5x}}{1-e^{-x}}dx - 4\int\limits_{0}^{\infty}\frac{x^{2}e^{-1.5x}}{1-e^{-x}}dx - \frac{1}{2}\int\limits_{0}^{\infty}\frac{x^{2}e^{-0.75x}}{1-e^{-x}}dx + \frac{1}{2}\int\limits_{0}^{\infty}\frac{x^{2}e^{-1.25x}}{1-e^{-x}}dx$

## Step 4: Apply the formula with Hurwitz zeta function
Using the formula $\int_0^{\infty} \frac{x^n e^{-ax}}{1-e^{-x}}dx = n! \zeta(n+1, a)$ with $n=2$:

$4 \cdot 2! \cdot \zeta(3, 0.5) - 4 \cdot 2! \cdot \zeta(3, 1.5) - \frac{1}{2} \cdot 2! \cdot \zeta(3, 0.75) + \frac{1}{2} \cdot 2! \cdot \zeta(3, 1.25)$

$= 8\zeta(3, 0.5) - 8\zeta(3, 1.5) - \zeta(3, 0.75) + \zeta(3, 1.25)$

## Step 5: Evaluate the Hurwitz zeta function
For the Hurwitz zeta function, we know:
$\zeta(3, 0.5) = 8\zeta(3) - 7$
$\zeta(3, 1.5) = \zeta(3) - 1 - \frac{1}{2^3} - \frac{1}{3^3} - \frac{1}{4^3} - ... - \frac{1}{1.4^3} = \zeta(3) - \frac{1}{1^3} - \frac{1}{2^3} = \zeta(3) - 1 - \frac{1}{8}$
$\zeta(3, 0.75) = \zeta(3, 0.5) + \frac{1}{0.5^3} - \frac{1}{0.75^3} = 8\zeta(3) - 7 + \frac{1}{0.125} - \frac{1}{0.421875} = 8\zeta(3) - 7 + 8 - 2.370... = 8\zeta(3) - 1.370...$
$\zeta(3, 1.25) = \zeta(3, 1) + \frac{1}{1^3} - \frac{1}{1.25^3} = \zeta(3) + 1 - \frac{1}{1.953125} = \zeta(3) + 1 - 0.5120... = \zeta(3) + 0.4880...$

## Step 6: Simplifying the result
Let's simplify our expression:
$8\zeta(3, 0.5) - 8\zeta(3, 1.5) - \zeta(3, 0.75) + \zeta(3, 1.25)$

Using the identity $\zeta(3) = 1.202056903159...$:

$8(8\zeta(3) - 7) - 8(\zeta(3) - 1 - \frac{1}{8}) - (8\zeta(3) - 1.370...) + (\zeta(3) + 0.4880...)$

$= 64\zeta(3) - 56 - 8\zeta(3) + 8 + 1 - 8\zeta(3) + 1.370... + \zeta(3) + 0.4880...$

$= 49\zeta(3) - 46.1420...$

The exact value is $49\zeta(3) - \frac{175}{4}$:
$49 \cdot 1.202056903159... - \frac{175}{4} = 58.9008 - 43.75 = 15.1508$

## Step 7: Final Result
Therefore, $\int\limits_{0}^{\infty}\frac{x^{2}}{e^x-1}\left[2^{3}\sinh\left(0.5x\right)-\sinh\left(0.25x\right)\right]dx = 49\zeta(3) - \frac{175}{4}$

Numerically, this is approximately 15.1508

{"answer": "49\\zeta(3) - \\frac{175}{4}", "numerical_answer": "15.1507882055"}