To solve the definite integral \(\int_{-4}^4 |x^3 - x| \, dx\), we need to handle the absolute value function carefully. The expression inside the absolute value, \(x^3 - x\), changes sign at the points where \(x^3 - x = 0\). Let's find these points:

\[ x^3 - x = x(x^2 - 1) = x(x - 1)(x + 1) = 0 \]

So, the roots are \(x = -1\), \(x = 0\), and \(x = 1\). These points divide the interval \([-4, 4]\) into four subintervals: \([-4, -1]\), \([-1, 0]\), \([0, 1]\), and \([1, 4]\).

We need to determine the sign of \(x^3 - x\) in each of these intervals:

1. For \(x \in [-4, -1]\):
   - \(x^3 - x\) is positive because \(x^3\) is negative and \(x\) is negative, making \(x^3 - x\) positive.
   - Therefore, \(|x^3 - x| = x^3 - x\).

2. For \(x \in [-1, 0]\):
   - \(x^3 - x\) is negative because \(x^3\) is negative and \(x\) is negative, making \(x^3 - x\) negative.
   - Therefore, \(|x^3 - x| = -(x^3 - x) = -x^3 + x\).

3. For \(x \in [0, 1]\):
   - \(x^3 - x\) is negative because \(x^3\) is positive and \(x\) is positive, making \(x^3 - x\) negative.
   - Therefore, \(|x^3 - x| = -(x^3 - x) = -x^3 + x\).

4. For \(x \in [1, 4]\):
   - \(x^3 - x\) is positive because \(x^3\) is positive and \(x\) is positive, making \(x^3 - x\) positive.
   - Therefore, \(|x^3 - x| = x^3 - x\).

Now, we can split the integral into four parts:

\[ \int_{-4}^4 |x^3 - x| \, dx = \int_{-4}^{-1} (x^3 - x) \, dx + \int_{-1}^{0} (-x^3 + x) \, dx + \int_{0}^{1} (-x^3 + x) \, dx + \int_{1}^{4} (x^3 - x) \, dx \]

Let's compute each integral separately:

1. \(\int_{-4}^{-1} (x^3 - x) \, dx\):

\[ \int_{-4}^{-1} (x^3 - x) \, dx = \left[ \frac{x^4}{4} - \frac{x^2}{2} \right]_{-4}^{-1} \]

Evaluating at the bounds:

\[ \left( \frac{(-1)^4}{4} - \frac{(-1)^2}{2} \right) - \left( \frac{(-4)^4}{4} - \frac{(-4)^2}{2} \right) = \left( \frac{1}{4} - \frac{1}{2} \right) - \left( \frac{256}{4} - \frac{16}{2} \right) = \left( -\frac{1}{4} \right) - \left( 64 - 8 \right) = -\frac{1}{4} - 56 = -\frac{225}{4} \]

2. \(\int_{-1}^{0} (-x^3 + x) \, dx\):

\[ \int_{-1}^{0} (-x^3 + x) \, dx = \left[ -\frac{x^4}{4} + \frac{x^2}{2} \right]_{-1}^{0} \]

Evaluating at the bounds:

\[ \left( -\frac{0^4}{4} + \frac{0^2}{2} \right) - \left( -\frac{(-1)^4}{4} + \frac{(-1)^2}{2} \right) = 0 - \left( -\frac{1}{4} + \frac{1}{2} \right) = 0 - \left( \frac{1}{4} \right) = -\frac{1}{4} \]

3. \(\int_{0}^{1} (-x^3 + x) \, dx\):

\[ \int_{0}^{1} (-x^3 + x) \, dx = \left[ -\frac{x^4}{4} + \frac{x^2}{2} \right]_{0}^{1} \]

Evaluating at the bounds:

\[ \left( -\frac{1^4}{4} + \frac{1^2}{2} \right) - \left( -\frac{0^4}{4} + \frac{0^2}{2} \right) = \left( -\frac{1}{4} + \frac{1}{2} \right) - 0 = \frac{1}{4} \]

4. \(\int_{1}^{4} (x^3 - x) \, dx\):

\[ \int_{1}^{4} (x^3 - x) \, dx = \left[ \frac{x^4}{4} - \frac{x^2}{2} \right]_{1}^{4} \]

Evaluating at the bounds:

\[ \left( \frac{4^4}{4} - \frac{4^2}{2} \right) - \left( \frac{1^4}{4} - \frac{1^2}{2} \right) = \left( \frac{256}{4} - \frac{16}{2} \right) - \left( \frac{1}{4} - \frac{1}{2} \right) = \left( 64 - 8 \right) - \left( -\frac{1}{4} \right) = 56 + \frac{1}{4} = \frac{225}{4} \]

Now, summing all the integrals:

\[ \int_{-4}^4 |x^3 - x| \, dx = -\frac{225}{4} - \frac{1}{4} + \frac{1}{4} + \frac{225}{4} = 0 \]

The exact answer is:

\[ \boxed{0} \]

The numerical approximation of the result is:

\[ 0.0000000000 \]

Output in JSON format:

```json
{"answer": "\\boxed{0}", "numerical_answer": "0.0000000000"}
```