<think>
Okay, so I need to compute the definite integral from 0 to 2.0 of x^(-3/4) times (2.0 - x)^(-1/4) multiplied by the modified Bessel function I₁ of 1.0 times the fourth root of x(2.0 - x) dx. Hmm, that looks a bit complicated, but let's break it down step by step.

First, let me recall what I know about integrals involving Bessel functions. Modified Bessel functions of the first kind, I_n(z), often appear in solutions to certain differential equations, especially in cylindrical coordinates. The integral here has a product of power functions and a Bessel function, which might hint at a substitution to simplify the expression.

Looking at the integrand: x^(-3/4) * (2 - x)^(-1/4) * I₁(1.0 * (x(2 - x))^(1/4)). The exponents on x and (2 - x) are negative fractions, and the argument of the Bessel function is the fourth root of x(2 - x) multiplied by 1.0. Let me write that argument as (x(2 - x))^{1/4} = [x(2 - x)]^{1/4}.

Maybe a substitution can help here. Let's consider a substitution that simplifies the term under the fourth root. Let me set t = x/(2 - x). Wait, or maybe t = x(2 - x). Let me think. Alternatively, perhaps a trigonometric substitution? Since the limits are from 0 to 2, maybe x = 2 sin²θ or something like that. Let's try that.

Let’s try substituting x = 2 sin²θ. Then, when x = 0, θ = 0, and when x = 2, θ = π/2. Let's compute dx: dx = 4 sinθ cosθ dθ. Then, 2 - x = 2 - 2 sin²θ = 2 cos²θ. So, (2 - x) = 2 cos²θ. Then, x^(-3/4) becomes (2 sin²θ)^(-3/4) = 2^(-3/4) sin^(-3/2)θ. Similarly, (2 - x)^(-1/4) = (2 cos²θ)^(-1/4) = 2^(-1/4) cos^(-1/2)θ. 

The argument of the Bessel function is [x(2 - x)]^{1/4} = [2 sin²θ * 2 cos²θ]^{1/4} = [4 sin²θ cos²θ]^{1/4} = [ (2 sinθ cosθ)^2 ]^{1/4} = (2 sinθ cosθ)^{1/2} = sqrt(2 sinθ cosθ). Then, multiplying by 1.0, the argument becomes sqrt(2 sinθ cosθ). So, the Bessel function term is I₁(sqrt(2 sinθ cosθ)).

Putting all together, the integral becomes:

Integral from θ=0 to θ=π/2 of [2^(-3/4) sin^(-3/2)θ] * [2^(-1/4) cos^(-1/2)θ] * I₁(sqrt(2 sinθ cosθ)) * 4 sinθ cosθ dθ.

Let me compute the constants and simplify the terms:

2^(-3/4) * 2^(-1/4) = 2^(-1) = 1/2. Then, sin^(-3/2)θ * cos^(-1/2)θ * sinθ cosθ = sin^(-3/2 +1)θ * cos^(-1/2 +1)θ = sin^(-1/2)θ * cos^(1/2)θ. So, the integrand becomes (1/2) * 4 * sin^(-1/2)θ * cos^(1/2)θ * I₁(sqrt(2 sinθ cosθ)) dθ. The 1/2 * 4 is 2. So, 2 * sin^(-1/2)θ * cos^(1/2)θ * I₁(sqrt(2 sinθ cosθ)) dθ.

Simplify sin^(-1/2)θ * cos^(1/2)θ: that's (cosθ / sinθ)^(1/2) = cot^(1/2)θ. Hmm, not sure if that helps. Alternatively, sqrt(cosθ / sinθ) = sqrt(cotθ). Maybe another substitution here. Let's see.

Alternatively, let's look at the argument of the Bessel function: sqrt(2 sinθ cosθ) = sqrt(sin(2θ)) because sin(2θ) = 2 sinθ cosθ. Wait, sin(2θ) = 2 sinθ cosθ, so sqrt(2 sinθ cosθ) = sqrt(sin(2θ)). So, the argument is sqrt(sin(2θ)). Hmm, but the Bessel function is I₁(sqrt(sin(2θ))). Not sure if that helps.

Alternatively, maybe another substitution. Let me set u = sin(2θ). Then, du = 2 cos(2θ) dθ. But I don't see an immediate simplification. Alternatively, maybe set t = 2θ. Let's see.

Alternatively, perhaps express the integrand in terms of t = sqrt(2 sinθ cosθ). Let me see. Let t = sqrt(2 sinθ cosθ) = sqrt(sin(2θ)). Then, t^2 = sin(2θ). Differentiating both sides: 2t dt = 2 cos(2θ) dθ. So, t dt = cos(2θ) dθ. Hmm, but not sure if that helps.

Alternatively, perhaps there's a standard integral formula involving Bessel functions. Let me recall that integrals of the form ∫ x^ν e^{-α x} I_μ(β x) dx can sometimes be expressed in terms of hypergeometric functions, but I'm not sure. Alternatively, maybe there's an integral representation of the Bessel function that can be used here.

Wait, the modified Bessel function I₁(z) has an integral representation. For example, I₁(z) = (1/π) ∫_0^π e^{z cosθ} cosθ dθ. But I'm not sure if that helps here. Alternatively, maybe using generating functions or series expansions.

Alternatively, let's consider expanding the Bessel function in its power series. The modified Bessel function I₁(z) has the series expansion:

I₁(z) = Σ_{k=0}^∞ ( (z/2)^{2k +1} ) / (k! (k +1)! )

So, substituting z = sqrt(2 sinθ cosθ), which is sqrt(sin(2θ)), so z = [sin(2θ)]^{1/2}. Then, z/2 = [sin(2θ)]^{1/2}/2. Then, the series becomes:

Σ_{k=0}^∞ [ ( [sin(2θ)]^{1/2} / 2 )^{2k +1} ] / (k! (k +1)! ) = Σ_{k=0}^∞ [ sin(2θ)^{k + 1/2} ] / (2^{2k +1} k! (k +1)! ) )

But integrating term by term might be possible. Let's see if that's feasible.

So, the integral becomes:

2 ∫_0^{π/2} [cosθ / sinθ]^{1/2} * Σ_{k=0}^∞ [ sin(2θ)^{k + 1/2} ] / (2^{2k +1} k! (k +1)! ) ) dθ

Simplify the terms inside the integral. Let's note that sin(2θ) = 2 sinθ cosθ. So, sin(2θ)^{k + 1/2} = (2 sinθ cosθ)^{k + 1/2} = 2^{k + 1/2} sin^{k + 1/2}θ cos^{k + 1/2}θ.

Substituting back into the integral:

2 * Σ_{k=0}^∞ [2^{k + 1/2} sin^{k + 1/2}θ cos^{k + 1/2}θ] / (2^{2k +1} k! (k +1)! )) * [cosθ / sinθ]^{1/2} dθ

Simplify the constants and exponents:

First, 2 * 2^{k + 1/2} / 2^{2k +1} = 2^{1 + k + 1/2 - 2k -1} = 2^{ -k + 1/2 }.

Then, the exponents on sinθ and cosθ:

sin^{k + 1/2}θ * [cosθ / sinθ]^{1/2} * cos^{k + 1/2}θ = sin^{k + 1/2 - 1/2}θ * cos^{k + 1/2 + 1/2}θ = sin^{k}θ * cos^{k +1}θ.

So, putting it all together, the integral becomes:

Σ_{k=0}^∞ [2^{-k + 1/2} / (k! (k +1)! )) ] ∫_0^{π/2} sin^{k}θ cos^{k +1}θ dθ

Now, the integral ∫_0^{π/2} sin^{k}θ cos^{k +1}θ dθ can be expressed in terms of the Beta function. Recall that:

∫_0^{π/2} sin^{m}θ cos^{n}θ dθ = (1/2) B( (m +1)/2, (n +1)/2 ) )

Where B is the Beta function, and B(a,b) = Γ(a)Γ(b)/Γ(a + b).

Here, m = k, n = k +1. So,

∫_0^{π/2} sin^{k}θ cos^{k +1}θ dθ = (1/2) B( (k +1)/2, (k +2)/2 )

But the Beta function can be expressed using Gamma functions:

B( (k +1)/2, (k +2)/2 ) = Γ( (k +1)/2 ) Γ( (k +2)/2 ) / Γ( (k +1 + k +2)/2 ) = Γ( (k +1)/2 ) Γ( (k +2)/2 ) / Γ( (2k +3)/2 )

Hmm, but this might be simplified using properties of the Gamma function. Recall that Γ(z)Γ(z + 1/2) = 2^{1 - 2z} √π Γ(2z). This is the duplication formula.

Let’s check if that applies here. Let’s set z = (k +1)/2. Then, Γ(z) Γ(z + 1/2) = Γ( (k +1)/2 ) Γ( (k +1)/2 + 1/2 ) = Γ( (k +1)/2 ) Γ( (k +2)/2 ) = 2^{1 - 2z} √π Γ(2z) = 2^{1 - (k +1)} √π Γ(k +1) )

So, Γ( (k +1)/2 ) Γ( (k +2)/2 ) = 2^{ -k } √π Γ(k +1 )

Therefore, the Beta function becomes:

B( (k +1)/2, (k +2)/2 ) = [2^{-k} √π Γ(k +1 ) ] / Γ( (2k +3)/2 )

But Γ(k +1 ) = k! So,

B(...) = 2^{-k} √π k! / Γ( (2k +3)/2 )

Therefore, the integral becomes:

(1/2) * [2^{-k} √π k! / Γ( (2k +3)/2 ) ]

Putting this back into the series expression:

Σ_{k=0}^∞ [2^{-k + 1/2} / (k! (k +1)! )) ] * [ (1/2) * 2^{-k} √π k! / Γ( (2k +3)/2 ) ) ]

Simplify term by term:

First, constants: 2^{-k + 1/2} * (1/2) * 2^{-k} √π = 2^{-2k + 1/2 -1} √π = 2^{-2k -1/2} √π

Then, the k! cancels with the denominator's k!:

So, denominator is (k! (k +1)! ), numerator has k!, so we have 1/(k +1)! )

So, the term becomes:

2^{-2k -1/2} √π / ( (k +1)! Γ( (2k +3)/2 ) )

But √π = 2^{1/2} Γ(1/2), but not sure if that helps. Alternatively, let's see if Γ( (2k +3)/2 ) can be expressed in terms of factorials or other Gamma functions.

Note that (2k +3)/2 = k + 3/2. So, Γ(k + 3/2) = (k + 1/2) Γ(k + 1/2). And Γ(k + 1/2) can be expressed using the double factorial or other identities. Specifically, Γ(k + 1/2) = (2k)! √π / (4^k k! )

Wait, let's recall that:

Γ(n + 1/2) = (2n)! / (4^n n! ) √π for integer n ≥ 0.

So, Γ(k + 1/2) = (2k)! / (4^k k! ) √π. Then, Γ(k + 3/2) = (k + 1/2) Γ(k + 1/2) = (k + 1/2) * (2k)! / (4^k k! ) √π.

But let's compute Γ(k + 3/2):

Γ(k + 3/2) = (k + 1/2) Γ(k + 1/2) = (k + 1/2)(k - 1/2)...(1/2) Γ(1/2) = product from i=0 to k of (1/2 + i) ) * √π.

Alternatively, perhaps using the relation Γ(k + 3/2) = (2k + 2)! / (4^{k +1} (k +1)! )) √π. Wait, let's check for k=0: Γ(3/2) = (1/2)√π. If k=0, then (2*0 +2)! = 2! = 2, 4^{0 +1} =4, (0 +1)! =1, so 2/(4*1) √π = (2/4)√π = (1/2)√π, which matches. So yes, Γ(k + 3/2) = (2k + 2)! / (4^{k +1} (k +1)! )) √π.

Therefore, substituting back into the term:

Γ(k + 3/2) = (2k + 2)! / (4^{k +1} (k +1)! )) √π.

So, substituting into the term:

2^{-2k -1/2} √π / ( (k +1)! Γ(k + 3/2 ) ) = 2^{-2k -1/2} √π / [ (k +1)! * (2k + 2)! / (4^{k +1} (k +1)! )) √π ) ]

Simplify denominator:

Denominator: (k +1)! * (2k + 2)! / (4^{k +1} (k +1)! )) √π ) = (2k + 2)! / (4^{k +1} ) √π )

So, the term becomes:

2^{-2k -1/2} √π / [ (2k + 2)! / (4^{k +1} ) √π ) ] = 2^{-2k -1/2} √π * 4^{k +1} / (2k + 2)! ) * 1/√π

The √π cancels out:

= 2^{-2k -1/2} * 4^{k +1} / (2k + 2)! )

But 4^{k +1} = 2^{2(k +1)} = 2^{2k +2}, so:

= 2^{-2k -1/2} * 2^{2k +2} / (2k + 2)! ) = 2^{ (-2k -1/2) + 2k +2 } / (2k +2)! )

Simplify exponent: (-2k -1/2 +2k +2) = (3/2). So, 2^{3/2} / (2k +2)! )

Therefore, the term simplifies to 2^{3/2} / (2k +2)! )

So, the entire series becomes:

Σ_{k=0}^∞ [2^{3/2} / (2k +2)! ) ]

But wait, let's check the steps again because this seems too simplified. Wait, the term after substitution was:

2^{-2k -1/2} * 4^{k +1} / (2k +2)! )

Which is 2^{-2k -1/2} * (2^2)^{k +1} / (2k +2)! ) = 2^{-2k -1/2 + 2k +2} / (2k +2)! )

= 2^{3/2} / (2k +2)! )

Yes, that's correct. So, the series is Σ_{k=0}^∞ 2^{3/2} / (2k +2)! )

But wait, this seems to be a constant series, but that can't be right. Wait, no, the term is actually 2^{3/2} / (2k +2)! ), but the sum is over k from 0 to ∞. So, but 2^{3/2} is a constant factor, so the sum becomes 2^{3/2} Σ_{k=0}^∞ 1/(2k +2)! )

But Σ_{k=0}^∞ 1/(2k +2)! ) = Σ_{m=1}^∞ 1/(2m)! ), where m = k +1. So, this is Σ_{m=1}^∞ 1/(2m)! ) = Σ_{m=0}^∞ 1/(2m)! ) - 1/0! = cosh(1) + sinh(1) / 2? Wait, no. Wait, the sum Σ_{m=0}^∞ x^{2m}/(2m)! ) = cosh(x). So, when x=1, Σ_{m=0}^∞ 1/(2m)! ) = cosh(1). Therefore, Σ_{m=1}^∞ 1/(2m)! ) = cosh(1) - 1.

Therefore, the sum becomes 2^{3/2} (cosh(1) -1 )

But wait, let's check:

Σ_{k=0}^∞ 1/(2k +2)! ) = Σ_{k=1}^∞ 1/(2k)! ) = cosh(1) -1. Because cosh(1) = Σ_{k=0}^∞ 1/(2k)! ), so subtracting the k=0 term (which is 1) gives cosh(1) -1.

Therefore, the integral becomes 2^{3/2} (cosh(1) -1 )

But wait, 2^{3/2} is 2*sqrt(2). So, 2*sqrt(2)*(cosh(1) -1 )

But cosh(1) = (e + e^{-1})/2 ≈ (2.71828 + 0.36788)/2 ≈ 1.54308. So, cosh(1) -1 ≈ 0.54308. Then, 2*sqrt(2)*0.54308 ≈ 2*1.4142*0.54308 ≈ 1.531. But let's compute it more accurately.

But wait, let's check the steps again. Because this seems to have lost track of the original integral. Wait, the original integral was transformed into a series which simplified to 2^{3/2} Σ_{k=0}^\infty 1/(2k +2)! ), which is 2^{3/2} (cosh(1) -1 ). Therefore, the value of the integral is 2^{3/2} (cosh(1) -1 )

But let's check the steps again to make sure.

Starting from the integral:

Original integral became, after substitution and series expansion, a sum over k of terms leading to 2^{3/2} / (2k +2)! ), summed over k from 0 to ∞. So, sum_{k=0}^∞ 1/(2k +2)! ) = sum_{m=1}^∞ 1/(2m)! ) = cosh(1) -1. Therefore, the integral is 2^{3/2} (cosh(1) -1 )

But wait, the original integral was equal to this series, which is equal to 2^{3/2} (cosh(1) -1 ). Therefore, the exact answer is 2^{3/2} (cosh(1) -1 )

But let's check if this makes sense. Let's compute the numerical value. 2^{3/2} is 2.8284271247. cosh(1) is approximately 1.5430806348. So, cosh(1) -1 ≈ 0.5430806348. Multiplying these gives 2.8284271247 * 0.5430806348 ≈ 1.536469248. So, approximately 1.536469248.

But let's check if this is correct. Alternatively, maybe there's a mistake in the substitution steps.

Wait, let's recap:

Original integral: ∫_0^2 x^{-3/4} (2 -x)^{-1/4} I₁( (x(2 -x))^{1/4} ) dx

Substitution x = 2 sin²θ, leading to integral in terms of θ, which after substitution and expansion became a series that simplified to 2^{3/2} (cosh(1) -1 )

But let's check if there's an alternative approach. Maybe using a substitution to make the integral resemble a standard form.

Alternatively, consider the integral might be related to the Beta function multiplied by a hypergeometric function. Alternatively, perhaps using the integral representation of the Bessel function.

Alternatively, let's consider another substitution. Let’s set t = x(2 -x). Then, when x=0, t=0; x=2, t=0. The maximum of t is at x=1, t=1*1=1. But integrating from 0 to 2, t goes from 0 to 1 and back to 0. That might complicate things. Alternatively, set u = t^{1/4} = [x(2 -x)]^{1/4}, but not sure.

Alternatively, let's consider the substitution y = x/2, so that the integral becomes from 0 to 1, with x = 2y, dx = 2 dy. Then, the integral becomes:

∫_0^1 (2y)^{-3/4} (2 - 2y)^{-1/4} I₁( (2y * 2(1 - y))^{1/4} ) * 2 dy

Simplify:

(2)^{-3/4} (2)^{-1/4} * 2 ∫_0^1 y^{-3/4} (1 - y)^{-1/4} I₁( (4y(1 - y))^{1/4} ) dy

Which is 2^{-3/4 -1/4 +1} ∫ ... dy = 2^{(-1) +1} = 2^0 =1. So, the integral becomes:

∫_0^1 y^{-3/4} (1 - y)^{-1/4} I₁( (4y(1 - y))^{1/4} ) dy

Hmm, not sure if that helps. The term inside the Bessel function is (4y(1 - y))^{1/4} = (4y(1 - y))^{1/4} = (4)^{1/4} (y(1 - y))^{1/4} = sqrt(2) (y(1 - y))^{1/4}

So, the argument is sqrt(2) (y(1 - y))^{1/4}

But this substitution doesn't seem to lead to a standard form either.

Alternatively, perhaps there's a relationship between this integral and the Beta function multiplied by a hypergeometric function. For example, integrals of the form ∫ x^{c-1} (1 -x)^{d -c -1} I_ν( (x(1 -x))^{1/2} ) dx from 0 to1 can sometimes be expressed in terms of hypergeometric functions, but I'm not sure.

Alternatively, perhaps using the integral representation of the Bessel function. For example, I₁(z) can be expressed as:

I₁(z) = \frac{1}{\pi} \int_0^\pi e^{z \cos \theta} \cos \theta d\theta

But substituting this into the integral might lead to a double integral which could be evaluated by switching the order of integration.

Let’s try that. Let’s write I₁( sqrt(2 sinθ cosθ) ) as per the integral representation:

I₁(z) = (1/π) ∫_0^π e^{z cosφ} cosφ dφ

So, substituting z = sqrt(2 sinθ cosθ), the original integral becomes:

2 ∫_0^{π/2} [cosθ / sinθ]^{1/2} * [ (1/π) ∫_0^π e^{ sqrt(2 sinθ cosθ) cosφ } cosφ dφ ] dθ

So, swapping the order of integration:

2/π ∫_0^π cosφ [ ∫_0^{π/2} [cosθ / sinθ]^{1/2} e^{ sqrt(2 sinθ cosθ) cosφ } dθ ] dφ

This seems complicated, but maybe changing variables in the inner integral. Let’s set t = sqrt(2 sinθ cosθ). Let’s see:

Let t = sqrt(2 sinθ cosθ) = sqrt(sin(2θ)). Then, t^2 = sin(2θ). Differentiating both sides: 2t dt = 2 cos(2θ) dθ => t dt = cos(2θ) dθ. But θ is from 0 to π/2, so 2θ is from 0 to π. Hmm, not sure.

Alternatively, set u = sinθ. Then, du = cosθ dθ. But θ from 0 to π/2, u from 0 to1. Then, cosθ = sqrt(1 - u^2). But the integrand has [cosθ / sinθ]^{1/2} = [sqrt(1 - u^2)/u]^{1/2} = (1 - u^2)^{1/4} u^{-1/2}

But the exponent is sqrt(2 u sqrt(1 - u^2)) cosφ. Hmm, not sure.

Alternatively, perhaps another substitution. Let’s set t = sinθ. Then, θ from 0 to π/2, t from 0 to1. Then, cosθ = sqrt(1 - t^2), dθ = dt / sqrt(1 - t^2). Then, the inner integral becomes:

∫_0}^{1} [ sqrt(1 - t^2)/t ]^{1/2} e^{ sqrt(2 t sqrt(1 - t^2)) cosφ } * dt / sqrt(1 - t^2)

Simplify:

[ (1 - t^2)^{1/2} / t ]^{1/2} = (1 - t^2)^{1/4} t^{-1/2}

Multiply by 1/sqrt(1 - t^2):

(1 - t^2)^{1/4} t^{-1/2} * (1 - t^2)^{-1/2} = (1 - t^2)^{-1/4} t^{-1/2}

So, the inner integral becomes:

∫_0^1 t^{-1/2} (1 - t^2)^{-1/4} e^{ sqrt(2 t sqrt(1 - t^2)) cosφ } dt

This still looks complicated. Maybe another substitution. Let’s set v = t^2. Then, dv = 2t dt => dt = dv/(2 sqrt(v)). Then, t^{-1/2} = v^{-1/4}, and sqrt(2 t sqrt(1 - t^2)) = sqrt(2 sqrt(v) sqrt(1 - v)) ) = (2)^{1/2} (v(1 - v))^{1/4}

So, the integral becomes:

∫_0^1 v^{-1/4} (1 - v)^{-1/4} e^{ 2^{1/2} (v(1 - v))^{1/4} cosφ } * dv/(2 v^{1/2} )

Simplify:

(1/2) ∫_0^1 v^{-3/4} (1 - v)^{-1/4} e^{ 2^{1/2} (v(1 - v))^{1/4} cosφ } dv

This still seems difficult. Perhaps this approach isn't the best.

Going back to the previous result where the integral was evaluated as 2^{3/2} (cosh(1) -1 ). Let's check if this makes sense numerically.

Compute 2^{3/2} (cosh(1) -1 ):

2^{3/2} = 2.8284271247461903

cosh(1) = (e + 1/e)/2 ≈ (2.718281828459045 + 0.3678794411714423)/2 ≈ 1.543080634815244

cosh(1) -1 ≈ 0.543080634815244

Multiply by 2.8284271247461903: 0.543080634815244 * 2.8284271247461903 ≈

Let me compute this:

0.5 * 2.828427 ≈ 1.4142135

0.0430806348 * 2.828427 ≈ 0.0430806348 * 2.828427 ≈ approximately 0.043 * 2.828 ≈ 0.1216

So total ≈ 1.4142 + 0.1216 ≈ 1.5358

So approximately 1.5358. Let's compute more accurately:

0.543080634815244 * 2.8284271247461903:

First, 0.5 * 2.8284271247461903 = 1.4142135623730951

0.043080634815244 * 2.8284271247461903:

0.04 * 2.8284271247461903 = 0.11313708498984761

0.003080634815244 * 2.8284271247461903 ≈ 0.0030806348 * 2.8284271247 ≈ 0.008714

So total ≈ 0.11313708498984761 + 0.008714 ≈ 0.12185108498984761

Adding to 1.4142135623730951: 1.4142135623730951 + 0.12185108498984761 ≈ 1.5360646473629427

So approximately 1.5360646474.

Now, let's compare this with a numerical approximation of the original integral. Let's use numerical integration to check.

The original integral is ∫_0^2 x^{-3/4} (2 -x)^{-1/4} I₁( (x(2 -x))^{1/4} ) dx.

Let's approximate this numerically. However, since I can't compute this here, I'll have to rely on the analytical result. But given that the steps led us to 2^{3/2} (cosh(1) -1 ), which is approximately 1.53606, and if that's the numerical result, then that's the answer.

But wait, let's check if there's a possible mistake in the substitution steps. For example, when we did the substitution x = 2 sin²θ, dx = 4 sinθ cosθ dθ. Then, the integrand became:

x^{-3/4} (2 -x)^{-1/4} I₁(...) dx

Which after substitution became:

(2 sin²θ)^{-3/4} (2 cos²θ)^{-1/4} I₁( sqrt(2 sinθ cosθ) ) *4 sinθ cosθ dθ

Which simplifies to:

2^{-3/4} sin^{-3/2}θ * 2^{-1/4} cos^{-1/2}θ * 4 sinθ cosθ * I₁(...) dθ

Which is 2^{-3/4 -1/4} * 4 * sin^{-3/2 +1}θ * cos^{-1/2 +1}θ * I₁(...) dθ

Which is 2^{-1} *4 * sin^{-1/2}θ * cos^{1/2}θ * I₁(...) dθ = 2 * sin^{-1/2}θ cos^{1/2}θ * I₁(...) dθ

Then, expanding I₁ in series and proceeding as before. The steps seem correct.

Therefore, the analytical result is 2^{3/2} (cosh(1) -1 )

But let's express this in terms of exponentials. cosh(1) = (e + e^{-1})/2, so:

2^{3/2} ( (e + e^{-1})/2 -1 ) = 2^{3/2} ( (e + e^{-1} -2)/2 ) = 2^{1/2} (e + e^{-1} -2)/2^{0} ) = sqrt(2) (e + e^{-1} -2)/2

Wait, 2^{3/2} /2 = 2^{1/2} = sqrt(2). So, yes:

2^{3/2} (cosh(1) -1 ) = sqrt(2) (e + e^{-1} -2)/2 * 2^{3/2} /2 ?

Wait, no. Let's re-express:

cosh(1) -1 = (e + e^{-1})/2 -1 = (e + e^{-1} -2)/2

Therefore, 2^{3/2} (cosh(1) -1 ) = 2^{3/2} * (e + e^{-1} -2)/2 = 2^{1/2} (e + e^{-1} -2)/1 = sqrt(2) (e + e^{-1} -2)

But wait, that contradicts the previous numerical calculation. Wait, let's compute sqrt(2) (e + e^{-1} -2):

e ≈ 2.7182818284, e^{-1} ≈ 0.3678794412

e + e^{-1} ≈ 3.0861612696

3.0861612696 -2 = 1.0861612696

sqrt(2) * 1.0861612696 ≈ 1.41421356237 * 1.0861612696 ≈ 1.536464...

Which is approximately 1.536464, which matches the previous numerical result. So, the exact answer is sqrt(2) (e + e^{-1} -2 )

But wait, the previous steps led to 2^{3/2} (cosh(1) -1 ) = sqrt(2) (e + e^{-1} -2 )

Yes, because 2^{3/2} = 2*sqrt(2), and (cosh(1) -1 ) = (e + e^{-1} -2)/2. So, 2*sqrt(2) * (e + e^{-1} -2)/2 = sqrt(2) (e + e^{-1} -2 )

Therefore, the exact answer is sqrt(2) (e + e^{-1} -2 )

But this can be simplified further. Let's compute e + e^{-1} -2:

e + e^{-1} -2 = e + 1/e -2 ≈ 2.718281828459045 + 0.3678794411714423 -2 ≈ 1.0861612696304873

So, sqrt(2) * 1.0861612696304873 ≈ 1.536469189914211

So, the exact answer is sqrt(2) (e + 1/e -2 )

But can this be expressed in terms of sinh or cosh?

Yes, since e + e^{-1} = 2 cosh(1), so e + e^{-1} -2 = 2(cosh(1) -1 )

Therefore, sqrt(2) * 2(cosh(1) -1 ) / 2 = sqrt(2) (cosh(1) -1 )

Wait, no. Wait, e + e^{-1} -2 = 2(cosh(1) -1 )

Therefore, sqrt(2) (e + e^{-1} -2 ) = sqrt(2) * 2 (cosh(1) -1 ) = 2 sqrt(2) (cosh(1) -1 )

But earlier steps said the integral is 2^{3/2} (cosh(1) -1 ), which is 2*sqrt(2) (cosh(1) -1 ), which is the same as sqrt(2) (e + e^{-1} -2 )

Yes, because 2 sqrt(2) (cosh(1) -1 ) = 2 sqrt(2) * ( (e + e^{-1})/2 -1 ) = sqrt(2) (e + e^{-1} -2 )

So, both expressions are equivalent. Therefore, the exact answer can be written as either 2^{3/2} (cosh(1) -1 ) or sqrt(2) (e + e^{-1} -2 )

But which form is more standard? Probably the one with hyperbolic functions. So, 2^{3/2} (cosh(1) -1 )

But let's check if this is correct. Let's verify with a numerical integration.

Suppose we compute the original integral numerically. Let's approximate it using a numerical method.

The integrand is x^{-3/4} (2 -x)^{-1/4} I₁( (x(2 -x))^{1/4} ) from 0=0 to x1=2.

But integrating this numerically might be challenging due to the singularities at x=0 and x=2. At x=0, x^{-3/4} tends to infinity, but the integral is convergent because the exponent is -3/4, which is integrable over [0,2]. Similarly, (2 -x)^{-1/4} is also integrable.

But since I can't compute this here, I'll have to trust the analytical steps. Given that the substitution and series expansion led to the result 2^{3/2} (cosh(1) -1 ), which numerically is approximately 1.5364691899.

Therefore, the exact answer is 2^{3/2} (cosh(1) -1 ), and the numerical approximation is approximately 1.5364691899, which rounds to 1.5364691899 when rounded to 10 decimal places.

But let's check with another approach. Let's recall that the modified Bessel function I₁(z) can be related to certain integrals. For example, in some tables of integrals, we might find integrals of the form ∫ x^{μ-1} (1 -x)^{ν-1} I_λ (a x^{k} (1 -x)^{m}) dx, but I'm not sure.

Alternatively, perhaps using the generating function for Bessel functions. But given the time I've spent and the steps followed, I think the analytical result is correct.

Therefore, the final answer is 2^{3/2} (cosh(1) -1 ), which is 2*sqrt(2)*(cosh(1) -1 ), and numerically approximately 1.5364691899.
</think>

{"answer": "2^{\\frac{3}{2}} \\left( \\cosh(1) - 1 \\right)", "numerical_answer": 1.5364691899}