

To calculate the definite integral \(\int_0^{2\pi}\left|1+2\sin x\right|dx\), we first determine where the expression inside the absolute value, \(1 + 2\sin x\), is positive or negative. 

### Step 1: Find zeros of \(1 + 2\sin x\)
Solve \(1 + 2\sin x = 0\):
\[
\sin x = -\frac{1}{2}
\]
The solutions in \([0, 2\pi)\) are \(x = \frac{7\pi}{6}\) and \(x = \frac{11\pi}{6}\).

### Step 2: Split the integral based on sign changes
The function \(1 + 2\sin x\) is:
- Positive on \([0, \frac{7\pi}{6}) \cup [\frac{11\pi}{6}, 2\pi]\),
- Negative on \([\frac{7\pi}{6}, \frac{11\pi}{6}]\).

Thus, the integral splits into three parts:
\[
\int_0^{2\pi}\left|1+2\sin x\right|dx = \int_0^{\frac{7\pi}{6}} (1 + 2\sin x)dx + \int_{\frac{7\pi}{6}}^{\frac{11\pi}{6}} -(1 + 2\sin x)dx + \int_{\frac{11\pi}{6}}^{2\pi} (1 + 2\sin x)dx
\]

### Step 3: Evaluate each integral
The antiderivative of \(1 + 2\sin x\) is \(x - 2\cos x\), and the antiderivative of \(-(1 + 2\sin x)\) is \(-x + 2\cos x\).

1. **First integral (\([0, \frac{7\pi}{6}]\))**:
\[
\int_0^{\frac{7\pi}{6}} (1 + 2\sin x)dx = \left[x - 2\cos x\right]_0^{\frac{7\pi}{6}} = \left(\frac{7\pi}{6} - 2\cos\left(\frac{7\pi}{6}\right)\right) - \left(0 - 2\cos 0\right)
\]
Since \(\cos\left(\frac{7\pi}{6}\right) = -\frac{\sqrt{3}}{2}\) and \(\cos 0 = 1\):
\[
= \frac{7\pi}{6} + \sqrt{3} + 2
\]

2. **Second integral (\([\frac{7\pi}{6}, \frac{11\pi}{6}]\))**:
\[
\int_{\frac{7\pi}{6}}^{\frac{11\pi}{6}} -(1 + 2\sin x)dx = \left[-x + 2\cos x\right]_{\frac{7\pi}{6}}^{\frac{11\pi}{6}} = \left(-\frac{11\pi}{6} + 2\cos\left(\frac{11\pi}{6}\right)\right) - \left(-\frac{7\pi}{6} + 2\cos\left(\frac{7\pi}{6}\right)\right)
\]
Since \(\cos\left(\frac{11\pi}{6}\right) = \frac{\sqrt{3}}{2}\) and \(\cos\left(\frac{7\pi}{6}\right) = -\frac{\sqrt{3}}{2}\):
\[
= -\frac{2\pi}{3} + 2\sqrt{3}
\]

3. **Third integral (\([\frac{11\pi}{6}, 2\pi]\))**:
\[
\int_{\frac{11\pi}{6}}^{2\pi} (1 + 2\sin x)dx = \left[x - 2\cos x\right]_{\frac{11\pi}{6}}^{2\pi} = \left(2\pi - 2\cos 2\pi\right) - \left(\frac{11\pi}{6} - 2\cos\left(\frac{11\pi}{6}\right)\right)
\]
Since \(\cos 2\pi = 1\) and \(\cos\left(\frac{11\pi}{6}\right) = \frac{\sqrt{3}}{2}\):
\[
= \frac{\pi}{6} - 2 + \sqrt{3}
\]

### Step 4: Sum the results
Adding the three integrals:
\[
\left(\frac{7\pi}{6} + \sqrt{3} + 2\right) + \left(-\frac{2\pi}{3} + 2\sqrt{3}\right) + \left(\frac{\pi}{6} - 2 + \sqrt{3}\right) = \frac{2\pi}{3} + 4\sqrt{3}
\]

### Numerical Approximation
The exact result is \(\frac{2\pi}{3} + 4\sqrt{3}\). Numerically:
\[
\frac{2\pi}{3} \approx 2.0943951024, \quad 4\sqrt{3} \approx 6.9282032303
\]
Adding these gives:
\[
2.0943951024 + 6.9282032303 \approx 9.0225983327
\]

{"answer": "\\frac{2\\pi}{3} + 4\\sqrt{3}", "numerical_answer": "9.0225983327"}