

To solve the definite integral \(\int_0^1 \frac{e^{\arctan(x)}}{(x^2+1)^{3/2}} \, dx\), we proceed with the following steps:

### Step 1: Substitution
Let \( t = \arctan(x) \). Then:
- \( x = \tan(t) \)
- \( dx = \sec^2(t) \, dt \)
- When \( x = 0 \), \( t = 0 \); when \( x = 1 \), \( t = \frac{\pi}{4} \).

### Step 2: Rewrite the Integral
The denominator \( (x^2 + 1)^{3/2} \) becomes \( (\tan^2(t) + 1)^{3/2} = (\sec^2(t))^{3/2} = \sec^3(t) \). The numerator \( e^{\arctan(x)} \) becomes \( e^t \). Substituting these into the integral:
\[
\int_0^1 \frac{e^{\arctan(x)}}{(x^2+1)^{3/2}} \, dx = \int_0^{\pi/4} \frac{e^t}{\sec^3(t)} \cdot \sec^2(t) \, dt = \int_0^{\pi/4} e^t \cos(t) \, dt
\]
(Here, \( \frac{1}{\sec^3(t)} \cdot \sec^2(t) = \cos(t) \).)

### Step 3: Evaluate the Integral
The integral \( \int e^t \cos(t) \, dt \) is a standard form. Using integration by parts or recognizing the antiderivative, we find:
\[
\int e^t \cos(t) \, dt = \frac{e^t (\cos(t) + \sin(t))}{2} + C
\]

### Step 4: Apply Limits of Integration
Evaluating from \( t = 0 \) to \( t = \frac{\pi}{4} \):
\[
\left. \frac{e^t (\cos(t) + \sin(t))}{2} \right|_0^{\pi/4} = \frac{e^{\pi/4} \left( \cos\left(\frac{\pi}{4}\right) + \sin\left(\frac{\pi}{4}\right) \right)}{2} - \frac{e^0 (\cos(0) + \sin(0))}{2}
\]
Since \( \cos\left(\frac{\pi}{4}\right) = \sin\left(\frac{\pi}{4}\right) = \frac{\sqrt{2}}{2} \) and \( \cos(0) = 1 \), \( \sin(0) = 0 \), this simplifies to:
\[
\frac{e^{\pi/4} \cdot \sqrt{2}}{2} - \frac{1}{2} = \frac{e^{\pi/4} \sqrt{2} - 1}{2}
\]

### Step 5: Numerical Approximation
Using \( e^{\pi/4} \approx 2.1932800507 \) and \( \sqrt{2} \approx 1.4142135624 \):
\[
\frac{e^{\pi/4} \sqrt{2} - 1}{2} \approx \frac{(2.1932800507 \cdot 1.4142135624) - 1}{2} \approx \frac{3.101766123 - 1}{2} \approx 1.0508830615
\]

### Final Answer
{"answer": "\\frac{e^{\\pi/4} \\sqrt{2} - 1}{2}", "numerical_answer": "1.0508830615"}