Let's proceed step by step.

Let's define the integral:
\[
I = \int_0^{2} x^{-3/4} (2-x)^{-1/4} I_1\big(1 \cdot [x(2-x)]^{1/4}\big) \, dx
\]
where \( I_1(z) \) is the modified Bessel function of the first kind, order 1.

## 1. Change of Variables

Let us consider the substitution:

Let \( x = 2t \), so \( dx = 2dt \), \( x=0 \to t=0 \), \( x=2 \to t=1 \).
Then \( 2-x = 2 - 2t = 2(1-t) \).
So
\[
x^{-3/4} = (2t)^{-3/4} = 2^{-3/4} t^{-3/4}
\]
\[
(2-x)^{-1/4} = [2(1-t)]^{-1/4} = 2^{-1/4} (1-t)^{-1/4}
\]
\[
[x(2-x)]^{1/4} = [2t \cdot 2(1-t)]^{1/4} = [4t(1-t)]^{1/4} = 4^{1/4} [t(1-t)]^{1/4} = 2^{1/2} [t(1-t)]^{1/4}
\]
So, the argument of \( I_1 \) becomes \( 1 \cdot 2^{1/2} [t(1-t)]^{1/4} = \sqrt{2}\, [t(1-t)]^{1/4} \).

The differential: \( dx = 2dt \).

Putting it all together:
\[
I = \int_0^1 2^{-3/4} t^{-3/4} 2^{-1/4}(1-t)^{-1/4} I_1\left(\sqrt{2}[t(1-t)]^{1/4}\right) \cdot 2dt
\]
\[
= 2^{-3/4-1/4+1} \int_0^1 t^{-3/4} (1-t)^{-1/4} I_1\left(\sqrt{2}[t(1-t)]^{1/4}\right) dt
\]
\[
-3/4 - 1/4 + 1 = -1/2 + 1 = 1/2
\]
So,
\[
I = 2^{1/2} \int_0^1 t^{-3/4} (1-t)^{-1/4} I_1\left(\sqrt{2}[t(1-t)]^{1/4}\right) dt
\]

## 2. Series Expansion of the Bessel Function

Recall:
\[
I_1(z) = \sum_{k=0}^\infty \frac{1}{k!\,\Gamma(k+2)} \left( \frac{z}{2} \right)^{2k+1}
\]

Plugging in \( z = \sqrt{2} [t(1-t)]^{1/4} \):

\[
I_1\left(\sqrt{2}[t(1-t)]^{1/4}\right) = \sum_{k=0}^\infty \frac{1}{k!\,\Gamma(k+2)} \left( \frac{\sqrt{2}[t(1-t)]^{1/4}}{2} \right)^{2k+1}
\]

\[
= \sum_{k=0}^\infty \frac{1}{k!\Gamma(k+2)} 2^{(2k+1)/2} \cdot 2^{-(2k+1)} [t(1-t)]^{(2k+1)/4}
\]

But \(2^{(2k+1)/2} \cdot 2^{-(2k+1)} = 2^{(2k+1)/2 - (2k+1)} = 2^{-(2k+1)/2}\)

So,
\[
I_1\left(\sqrt{2}[t(1-t)]^{1/4}\right) = \sum_{k=0}^\infty \frac{1}{k!\Gamma(k+2)} 2^{-(2k+1)/2} [t(1-t)]^{(2k+1)/4}
\]

Thus, the integrand is:
\[
t^{-3/4} (1-t)^{-1/4} [t(1-t)]^{(2k+1)/4} = t^{-3/4 + (2k+1)/4} (1-t)^{-1/4 + (2k+1)/4} = t^{k/2} (1-t)^{k/2}
\]

So the power of \( t \) is \( k/2 \), and of \( 1-t \) is \( k/2 \).

Therefore, the integral becomes:
\[
I = 2^{1/2} \sum_{k=0}^\infty \frac{2^{-(2k+1)/2}}{k!\Gamma(k+2)} \int_0^1 t^{k/2} (1-t)^{k/2} dt
\]

Recall the beta function:
\[
\int_0^1 t^{a-1} (1-t)^{b-1} dt = \mathrm{B}(a, b) = \frac{\Gamma(a)\Gamma(b)}{\Gamma(a+b)}
\]

Here, \( a = 1 + k/2 \), \( b = 1 + k/2 \).

Therefore,
\[
\int_0^1 t^{k/2} (1-t)^{k/2} dt = \frac{\Gamma(1 + k/2)^2}{\Gamma(2 + k)}
\]

Compile everything:
\[
I = 2^{1/2} \sum_{k=0}^\infty \frac{2^{-(2k+1)/2}}{k!\Gamma(k+2)} \cdot \frac{\Gamma(1 + k/2)^2}{\Gamma(2 + k)}
\]

Notice \(2^{1/2} \cdot 2^{-(2k+1)/2}=2^{-k}\):

\[
2^{1/2} \cdot 2^{-(2k+1)/2} = 2^{1/2-(2k+1)/2} = 2^{(-2k+1-1)/2} = 2^{-k}
\]

So the sum becomes:
\[
I = \sum_{k=0}^\infty \frac{2^{-k}\Gamma(1 + k/2)^2}{k!\Gamma(k+2)\Gamma(k+2)}
\]

But recall \( \Gamma(k+2) = (k+1)! \), so:

\[
I = \sum_{k=0}^\infty \frac{2^{-k} [\Gamma(1 + k/2)]^2}{k! [(k+1)!]^2}
\]

This is our closed form.

## 3. Compact Expression

In LaTeX,
\[
I = \sum_{k=0}^{\infty} \frac{2^{-k} [\Gamma(1 + k/2)]^2}{k! [(k+1)!]^2}
\]

## 4. Numerical Evaluation

Let's compute the first few terms for a good approximation.

- For \(k=0\):

\[
2^0=1, \quad \Gamma(1+0/2)=\Gamma(1)=1,\, k!=1
\]
\[
[(k+1)!]^2 = (1!)^2 = 1^2=1
\]
So,
\[
\text{Term}_0 = \frac{1\cdot 1^2}{1 \cdot 1^2} = 1
\]

- For \(k=1\):

\[
2^{-1}=1/2,\quad \Gamma(1+1/2)^2 = [\Gamma(3/2)]^2 = \left(\frac{\sqrt{\pi}}{2}\right)^2 = \frac{\pi}{4}
\]
\[
k!=1,\quad (k+1)!=2,\quad [(k+1)!]^2 = 4
\]
So,
\[
\text{Term}_1 = \frac{1}{2} \cdot \frac{\pi}{4} \frac{1}{1 \cdot 4} = \frac{\pi}{32} \approx 0.0981747704
\]

- For \(k=2\):

\[
2^{-2}=1/4,\quad \Gamma(1+1)^2=\Gamma(2)^2=1^2=1
\]
\[
k!=2,\quad (k+1)!=3,\quad 3^2=9
\]
So,
\[
\text{Term}_2 = \frac{1}{4} \cdot \frac{1}{2 \cdot 9} = \frac{1}{72} \approx 0.0138888889
\]

- For \(k=3\):

\[
2^{-3}=1/8,\quad \Gamma(1+1.5)^2 = [\Gamma(2.5)]^2 
\]
\[
\Gamma(2.5) = (1.5)\Gamma(1.5) = 1.5 \times 0.886226925 = 1.329340388
\]
\[
(1.329340388)^2 = 1.767262624
\]
\[
k!=6,\quad (k+1)!=4!,\quad 24^2=576
\]
So,
\[
\text{Term}_3 = \frac{1}{8} \cdot \frac{1.767262624}{6 \cdot 576} = \frac{1.767262624}{27648} \approx 0.0000639466
\]

- For \(k=4\):

\[
2^{-4}=1/16,\, \Gamma(1+2)^2 = \Gamma(3)^2 = (2)^2=4
\]
\[
k!=24,\, (k+1)!=5!=120,\, (120)^2=14400
\]
So,
\[
\text{Term}_4 = \frac{1}{16} \cdot \frac{4}{24 \cdot 14400} = \frac{4}{16 \cdot 24 \cdot 14400} = \frac{4}{5529600} \approx 0.0000007235
\]

- For \(k=5\):

\[
2^{-5}=1/32
\]
\[
\Gamma(1+2.5) = \Gamma(3.5) = 2.5 \Gamma(2.5) = 2.5 \times 1.329340388 \approx 3.32335097
\]
So squared: \( (3.32335097)^2 \approx 11.0437144 \)

\( k! = 120 \), \( (k+1)! = 720 \), so \( (k+1)!^2 = 518400 \)

Therefore,
\[
\text{Term}_5 = \frac{1}{32} \cdot \frac{11.0437144}{120 \cdot 518400} 
= \frac{11.0437144}{32 \times 120 \times 518400}= \frac{11.0437144}{1,990,656,000}
\approx 0.0000000055
\]

Add them up for partial sum:

\[
S \approx 1 + 0.0981747704 + 0.0138888889 + 0.0000639466 + 0.0000007235 + 0.0000000055 \approx 1.1121283349
\]

More generally, subsequent terms are negligible (decreasing rapidly).

So a good approximation to ten decimal places:
\[
\boxed{1.1121283349}
\]

## 5. Final JSON Output

```json
{"answer": "\\sum_{k=0}^{\\infty} \\frac{2^{-k} [\\Gamma(1 + k/2)]^2}{k! [(k+1)!]^2}", "numerical_answer": "1.1121283349"}
```