


To solve the definite integral \(\int_0^1 x^{-1/4}(1-x)^{1/4} I_1\left(\sqrt[4]{x(1-x)}\right) dx\), we proceed as follows:


### Step 1: Series Expansion of the Bessel Function
The modified Bessel function of the first kind \(I_1(z)\) has the series expansion:
\[
I_1(z) = \sum_{k=0}^\infty \frac{(z/2)^{2k+1}}{k! (k+1)!}
\]
Substituting \(z = \sqrt[4]{x(1-x)}\), we get:
\[
I_1\left(\sqrt[4]{x(1-x)}\right) = \sum_{k=0}^\infty \frac{\left(\sqrt[4]{x(1-x)}/2\right)^{2k+1}}{k! (k+1)!} = \sum_{k=0}^\infty \frac{x^{(2k+1)/4} (1-x)^{(2k+1)/4}}{2^{2k+1} k! (k+1)!}
\]


### Step 2: Substitute the Series into the Integral
The integrand becomes:
\[
x^{-1/4}(1-x)^{1/4} \cdot \sum_{k=0}^\infty \frac{x^{(2k+1)/4} (1-x)^{(2k+1)/4}}{2^{2k+1} k! (k+1)!} = \sum_{k=0}^\infty \frac{x^{k/2} (1-x)^{(k+1)/2}}{2^{2k+1} k! (k+1)!}
\]
Interchanging the sum and integral (justified by uniform convergence), the integral becomes:
\[
\sum_{k=0}^\infty \frac{1}{2^{2k+1} k! (k+1)!} \int_0^1 x^{k/2} (1-x)^{(k+1)/2} dx
\]


### Step 3: Evaluate the Integral Using the Beta Function
The integral \(\int_0^1 x^{k/2} (1-x)^{(k+1)/2} dx\) is a Beta function \(B\left(\frac{k}{2}+1, \frac{k+3}{2}\right)\), which relates to Gamma functions:
\[
B\left(a, b\right) = \frac{\Gamma(a)\Gamma(b)}{\Gamma(a+b)}
\]
Here, \(a = \frac{k}{2}+1\) and \(b = \frac{k+3}{2}\), so:
\[
\int_0^1 x^{k/2} (1-x)^{(k+1)/2} dx = \frac{\Gamma\left(\frac{k}{2}+1\right) \Gamma\left(\frac{k+3}{2}\right)}{\Gamma\left(k + \frac{5}{2}\right)}
\]


### Step 4: Simplify Using Gamma Function Properties
Using the duplication formula for Gamma functions and simplifying, the series reduces to a convergent sum. Evaluating the first few terms of the series numerically gives an approximation of the integral.


### Step 5: Numerical Approximation
Numerical integration (using adaptive quadrature) and summing the series terms yield a numerical approximation of the integral.


### Final Results
The exact answer involves an infinite series of Gamma functions, and the numerical approximation is approximately \(0.3503\).


{"answer": "\\sum_{k=0}^{\\infty} \\frac{\\Gamma\\left(\\frac{k}{2}+1\\right) \\Gamma\\left(\\frac{k+3}{2}\\right)}{2^{2k+1} k! (k+1)! \\Gamma\\left(k + \\frac{5}{2}\\right)}", "numerical_answer": "0.3503000000"}