<think>
Okay, so I need to compute the definite integral from 0 to 1 of x^(-1/2) times [1 - sqrt(x(1 - x))]^(-5/2) dx. Hmm, that looks a bit complicated, but maybe I can simplify it with a substitution. Let me start by writing down the integral again to make sure I have it right:

∫₀¹ x^(-1/2) [1 - √(x(1 - x))]^(-5/2) dx.

First, let me see if there's a substitution that can make this integral more manageable. The term inside the brackets is 1 minus the square root of x(1 - x). Maybe a trigonometric substitution? Or perhaps a beta function or gamma function approach? Since the limits are from 0 to 1, which is the interval for beta functions, that might be a good direction.

The beta function is defined as B(a, b) = ∫₀¹ t^(a-1)(1 - t)^(b-1) dt, which is related to the gamma function by B(a, b) = Γ(a)Γ(b)/Γ(a + b). But the integrand here is x^(-1/2) times [1 - sqrt(x(1 - x))]^(-5/2). Let me see if I can manipulate the expression inside the brackets to resemble something like (1 - t)^k.

Wait, let's try a substitution. Let me set t = sqrt(x(1 - x)). Then, maybe express x in terms of t. But solving for x might be complicated. Alternatively, maybe set x = sin²θ? Let's try that. If x = sin²θ, then dx = 2 sinθ cosθ dθ. Let's see:

When x = 0, θ = 0. When x = 1, θ = π/2. Then, substituting into the integral:

x^(-1/2) becomes (sin²θ)^(-1/2) = 1/sinθ.

sqrt(x(1 - x)) becomes sqrt(sin²θ (1 - sin²θ)) = sqrt(sin²θ cos²θ) = sinθ cosθ.

So the term inside the brackets becomes 1 - sinθ cosθ. Therefore, [1 - sinθ cosθ]^(-5/2).

Putting it all together, the integral becomes:

∫₀^(π/2) [1/sinθ] * [1 - sinθ cosθ]^(-5/2) * 2 sinθ cosθ dθ.

Simplify the terms:

The 1/sinθ and sinθ cancel out, leaving 2 cosθ. So the integral is:

2 ∫₀^(π/2) cosθ [1 - sinθ cosθ]^(-5/2) dθ.

Hmm, that's still a bit complicated. Let me see if I can simplify the expression 1 - sinθ cosθ. Maybe use a trigonometric identity. Remember that sinθ cosθ = (1/2) sin2θ. So 1 - (1/2) sin2θ. But I'm not sure if that helps. Alternatively, maybe express 1 - sinθ cosθ in terms of another trigonometric function. Let's see:

Alternatively, perhaps another substitution. Let me set u = sinθ. Then du = cosθ dθ. But θ goes from 0 to π/2, so u goes from 0 to 1. Then, substituting:

The integral becomes 2 ∫₀¹ [1 - u cosθ]^(-5/2) du. Wait, but cosθ is sqrt(1 - u²). So:

2 ∫₀¹ [1 - u sqrt(1 - u²)]^(-5/2) du. Hmm, that seems more complicated. Maybe not the best approach.

Let me think again. The original integral after substitution became 2 ∫₀^(π/2) cosθ [1 - sinθ cosθ]^(-5/2) dθ. Maybe another substitution here. Let me set t = sinθ. Then dt = cosθ dθ. Then θ from 0 to π/2 becomes t from 0 to 1. Then the integral becomes:

2 ∫₀¹ [1 - t sqrt(1 - t²)]^(-5/2) dt. Wait, that's similar to what I had before. Hmm, not helpful.

Alternatively, maybe expand [1 - sinθ cosθ]^(-5/2) using a series expansion? But that might not lead to an exact result. Alternatively, perhaps another substitution. Let me consider the term 1 - sinθ cosθ. Let's write it as 1 - (1/2) sin2θ. Then, 1 - (1/2) sin2θ. Maybe use a substitution for 2θ, but not sure.

Alternatively, perhaps use hypergeometric functions? But the problem says to compute the integral analytically, so maybe there's a way to express it in terms of beta or gamma functions. Let me check the form again.

Wait, let's try another substitution. Let me go back to the original integral:

∫₀¹ x^(-1/2) [1 - sqrt(x(1 - x))]^(-5/2) dx.

Let me set x = sin²θ, as before. Then, as before, the integral becomes 2 ∫₀^(π/2) cosθ [1 - sinθ cosθ]^(-5/2) dθ. Let me see if I can manipulate 1 - sinθ cosθ. Let's write it as 1 - (1/2) sin2θ. Wait, sinθ cosθ = (1/2) sin2θ. So 1 - (1/2) sin2θ. Hmm. So the integral becomes 2 ∫₀^(π/2) cosθ [1 - (1/2) sin2θ]^(-5/2) dθ.

Alternatively, maybe set φ = 2θ. Then when θ = 0, φ = 0; θ = π/2, φ = π. Then dφ = 2 dθ, so dθ = dφ/2. Then the integral becomes:

2 ∫₀^π cos(φ/2) [1 - (1/2) sinφ]^(-5/2) * (dφ/2).

Wait, cosθ = cos(φ/2). So the integral becomes:

(2 * 1/2) ∫₀^π cos(φ/2) [1 - (1/2) sinφ]^(-5/2) dφ = ∫₀^π cos(φ/2) [1 - (1/2) sinφ]^(-5/2) dφ.

Hmm, not sure. Maybe another substitution. Let me consider t = φ/2. Then φ = 2t, dφ = 2dt. Then the integral becomes:

∫₀^(π/2) cos t [1 - (1/2) sin(2t)]^(-5/2) * 2 dt.

But sin(2t) = 2 sin t cos t, so:

1 - (1/2)(2 sin t cos t) = 1 - sin t cos t. Wait, that's the same expression as before. So this substitution doesn't help. Hmm.

Alternatively, perhaps use a substitution where u = sin t. Let me try that. Let u = sin t, then du = cos t dt. Then t from 0 to π/2 becomes u from 0 to 1. Then the integral becomes:

2 ∫₀¹ [1 - u sqrt(1 - u²)]^(-5/2) du. Wait, this seems like a loop. Maybe I need a different approach.

Let me go back to the original integral. Let's consider substitution y = sqrt(x(1 - x)). Then y² = x(1 - x). Let me see if I can express x in terms of y. y² = x - x², so x² - x + y² = 0. Solving for x: x = [1 ± sqrt(1 - 4y²)] / 2. Hmm, but this might complicate things. Alternatively, perhaps use substitution t = sqrt(x/(1 - x)). Let me try that.

Let t = sqrt(x/(1 - x)). Then t² = x/(1 - x) => x = t²/(1 + t²). Then dx/dt = [2t(1 + t²) - t²(2t)]/(1 + t²)^2 = [2t + 2t³ - 2t³]/(1 + t²)^2 = 2t/(1 + t²)^2.

The limits: when x = 0, t = 0; when x = 1, t approaches infinity. So the integral becomes:

∫₀^∞ [ (t²/(1 + t²))^(-1/2) ] * [1 - sqrt( (t²/(1 + t²))(1 - t²/(1 + t²)) ) ]^(-5/2) * [2t/(1 + t²)^2] dt.

Simplify each part:

First term: (t²/(1 + t²))^(-1/2) = (t²)^(-1/2) * (1 + t²)^(1/2) = (1/t) * sqrt(1 + t²).

Second term: sqrt( (t²/(1 + t²))(1 - t²/(1 + t²)) ) = sqrt( t²/(1 + t²) * ( (1 + t² - t²)/(1 + t²) ) ) = sqrt( t²/(1 + t²) * 1/(1 + t²) ) = sqrt( t²/(1 + t²)^2 ) = t/(1 + t²).

So the term inside the brackets becomes 1 - t/(1 + t²) = (1 + t² - t)/(1 + t²) = (t² - t + 1)/(1 + t²). Therefore, [1 - sqrt(x(1 - x))]^(-5/2) becomes [ (t² - t + 1)/(1 + t²) ]^(-5/2) = (1 + t²)^(5/2) / (t² - t + 1)^(5/2).

Putting it all together, the integral becomes:

∫₀^∞ [ (1/t) sqrt(1 + t²) ] * [ (1 + t²)^(5/2) / (t² - t + 1)^(5/2) ] * [2t/(1 + t²)^2] dt.

Simplify term by term:

First term: (1/t) sqrt(1 + t²) = (1/t)(1 + t²)^(1/2).

Second term: (1 + t²)^(5/2) / (t² - t + 1)^(5/2).

Third term: 2t/(1 + t²)^2.

Multiply them all:

(1/t)(1 + t²)^(1/2) * (1 + t²)^(5/2) / (t² - t + 1)^(5/2) * 2t/(1 + t²)^2.

Combine exponents of (1 + t²):

1/2 + 5/2 - 2 = (6/2 - 2) = 3 - 2 = 1. So (1 + t²)^1.

The t terms: (1/t) * 2t = 2.

So the integral simplifies to:

2 ∫₀^∞ (1 + t²) / (t² - t + 1)^(5/2) dt.

Hmm, that's a bit simpler. Now, the integral is 2 ∫₀^∞ (1 + t²)/(t² - t + 1)^(5/2) dt. Let me see if I can simplify the denominator. The denominator is (t² - t + 1)^(5/2). Let's complete the square for the quadratic in the denominator:

t² - t + 1 = t² - t + (1/4) + 3/4 = (t - 1/2)^2 + 3/4. So it's a quadratic with vertex at t = 1/2 and a minimum of 3/4. Not sure if that helps, but maybe a substitution here. Let me set u = t - 1/2. Then t = u + 1/2, dt = du. The integral becomes:

2 ∫_{-1/2}^∞ [ ( (u + 1/2)^2 + 1 ) / (u² + 3/4)^(5/2) ] du.

Wait, expanding (u + 1/2)^2 + 1:

(u² + u + 1/4) + 1 = u² + u + 5/4.

So the integral becomes:

2 ∫_{-1/2}^∞ (u² + u + 5/4) / (u² + 3/4)^(5/2) du.

Hmm, this might not be helpful. Alternatively, perhaps split the numerator:

(1 + t²) = (t² - t + 1) + t. So:

(1 + t²) = (t² - t + 1) + t. Then the integral becomes:

2 ∫₀^∞ [ (t² - t + 1) + t ] / (t² - t + 1)^(5/2) dt = 2 ∫₀^∞ [1/(t² - t + 1)^(3/2) + t/(t² - t + 1)^(5/2)] dt.

Maybe split the integral into two parts:

2 [ ∫₀^∞ 1/(t² - t + 1)^(3/2) dt + ∫₀^∞ t/(t² - t + 1)^(5/2) dt ].

Let me handle each integral separately. Let's call the first integral I1 and the second I2.

For I1: ∫₀^∞ 1/(t² - t + 1)^(3/2) dt.

Let me complete the square again: t² - t + 1 = (t - 1/2)^2 + 3/4. Let me set u = t - 1/2, then du = dt. The limits become from u = -1/2 to u = ∞.

So I1 = ∫_{-1/2}^∞ 1/(u² + 3/4)^(3/2) du.

The integral of 1/(u² + a²)^(3/2) du is u/(a² sqrt(u² + a²)) ) + C. Wait, let me check:

Let me recall that ∫ du/(u² + a²)^(3/2) = u/(a² sqrt(u² + a²)) ) + C. Yes, that's correct. So applying this formula with a² = 3/4, so a = sqrt(3)/2.

Therefore, I1 = [ u/( (3/4) sqrt(u² + 3/4) ) ) ] evaluated from u = -1/2 to u = ∞.

At u = ∞, the term becomes [ ∞ / ( (3/4) * ∞ ) ] = 1/(3/4) = 4/3. At u = -1/2:

[ (-1/2) / ( (3/4) sqrt( (1/2)^2 + 3/4 ) ) ) ] = (-1/2) / ( (3/4) sqrt(1/4 + 3/4) ) = (-1/2) / ( (3/4) * 1 ) ) = (-1/2) * (4/3) = -2/3.

Therefore, I1 = [4/3 - (-2/3)] = 4/3 + 2/3 = 6/3 = 2.

Now, moving to I2: ∫₀^∞ t/(t² - t + 1)^(5/2) dt.

Again, complete the square: t² - t + 1 = (t - 1/2)^2 + 3/4. Let u = t - 1/2, so t = u + 1/2, dt = du. The limits become u = -1/2 to u = ∞.

So I2 = ∫_{-1/2}^∞ (u + 1/2)/ (u² + 3/4)^(5/2) du.

Split this into two integrals:

I2 = ∫_{-1/2}^∞ u/(u² + 3/4)^(5/2) du + (1/2) ∫_{-1/2}^∞ 1/(u² + 3/4)^(5/2) du.

Let's compute each part separately. Let's call the first integral I2a and the second I2b.

For I2a: ∫ u/(u² + 3/4)^(5/2) du.

Let me make a substitution: let v = u² + 3/4, then dv = 2u du, so (1/2) dv = u du. Then I2a becomes (1/2) ∫ v^(-5/2) dv. The limits: when u = -1/2, v = (-1/2)^2 + 3/4 = 1/4 + 3/4 = 1. When u approaches ∞, v approaches ∞.

So I2a = (1/2) ∫₁^∞ v^(-5/2) dv = (1/2) [ (-2/3) v^(-3/2) ] from 1 to ∞.

Evaluating at ∞: (-2/3)(0) = 0. At 1: (-2/3)(1) = -2/3. So I2a = (1/2)(0 - (-2/3)) = (1/2)(2/3) = 1/3.

Now, I2b: (1/2) ∫_{-1/2}^∞ 1/(u² + 3/4)^(5/2) du.

The integral of 1/(u² + a²)^(5/2) du can be found using the formula:

∫ du/(u² + a²)^(5/2) = (1/(3a²)) * [ u/(a² (u² + a²)^(1/2)) ) + 2u/(3a² (u² + a²)^(3/2)) ) ] + C. Wait, maybe better to use a reduction formula or trigonometric substitution.

Alternatively, use substitution u = a tanθ. Let a = sqrt(3)/2, so u = (sqrt(3)/2) tanθ, du = (sqrt(3)/2) sec²θ dθ. Then u² + a² = (3/4) tan²θ + 3/4 = (3/4)(tan²θ + 1) = (3/4) sec²θ. The integral becomes:

∫ (sqrt(3)/2 sec²θ dθ) / ( (3/4 sec²θ )^(5/2) ) = (sqrt(3)/2) ∫ sec²θ / ( (3/4)^(5/2) sec^5θ ) dθ.

Simplify:

( sqrt(3)/2 ) * (4/3)^(5/2) ∫ sec²θ / sec^5θ dθ = ( sqrt(3)/2 ) * (4/3)^(5/2) ∫ cos³θ dθ.

But this seems complicated. Alternatively, use the standard integral formula. Let me recall that:

∫ du/(u² + a²)^(n) du = (1/(2a²(n-1))) ) [ u/(u² + a²)^(n-1) ) + (2n - 3) ∫ du/(u² + a²)^(n-1) ) ].

But maybe for n = 5/2, which is not an integer. Hmm, this might not be straightforward. Alternatively, use substitution.

Wait, let's compute it directly. Let me set u = (sqrt(3)/2) tanθ, then du = (sqrt(3)/2) sec²θ dθ. Then the integral becomes:

∫ [ (sqrt(3)/2) sec²θ dθ ] / [ ( (3/4) sec²θ )^(5/2) ) ] = (sqrt(3)/2) ∫ sec²θ / ( (3/4)^(5/2) sec^5θ ) dθ.

Simplify the denominator:

(3/4)^(5/2) = (3^(5/2))/(4^(5/2)) ) = (3^2 * sqrt(3))/(2^5) ) = (9 sqrt(3))/32.

So the integral becomes:

(sqrt(3)/2) * (32)/(9 sqrt(3)) ) ∫ sec²θ / sec^5θ dθ = (sqrt(3)/2 * 32/(9 sqrt(3))) ) ∫ cos³θ dθ.

The sqrt(3) cancels, so:

(16/9) ∫ cos³θ dθ.

The integral of cos³θ dθ can be computed as:

∫ cos³θ dθ = ∫ cosθ (1 - sin²θ) dθ = ∫ cosθ dθ - ∫ cosθ sin²θ dθ = sinθ - (1/3) sin³θ + C.

Therefore, the integral becomes:

(16/9) [ sinθ - (1/3) sin³θ ] + C.

Now, we need to express θ in terms of u. Since u = (sqrt(3)/2) tanθ, then tanθ = (2u)/sqrt(3), so θ = arctan(2u/sqrt(3)). Therefore, sinθ = 2u / sqrt(4u² + 3). Wait, let's see:

If tanθ = (2u)/sqrt(3), then opposite side is 2u, adjacent is sqrt(3), hypotenuse is sqrt(4u² + 3). Therefore, sinθ = 2u / sqrt(4u² + 3).

Similarly, sin³θ = (2u)^3 / (4u² + 3)^(3/2).

Therefore, substituting back:

(16/9) [ (2u)/sqrt(4u² + 3) - (1/3)(8u³)/(4u² + 3)^(3/2) ) ] + C.

Simplify:

(16/9) [ (2u)/(4u² + 3)^(1/2) - (8u³)/(3(4u² + 3)^(3/2)) ) ].

Factor out 2u/(4u² + 3)^(3/2):

= (16/9) * 2u/(4u² + 3)^(3/2) [ (4u² + 3) - (4u²)/3 ].

Wait, let's compute the terms inside the brackets:

First term: (2u)/(4u² + 3)^(1/2) = 2u (4u² + 3)^(-1/2).

Second term: -(8u³)/(3(4u² + 3)^(3/2)) = - (8u³)/(3(4u² + 3)^(3/2)).

Let me factor out 2u/(4u² + 3)^(3/2):

= 2u/(4u² + 3)^(3/2) [ (4u² + 3) - (4u²)/3 ].

Wait, let's see:

First term: 2u/(4u² + 3)^(1/2) = 2u (4u² + 3)^(-1/2) = 2u (4u² + 3)^(-1/2) * (4u² + 3)/(4u² + 3) )

= 2u (4u² + 3) / (4u² + 3)^(3/2) )

= 2u (4u² + 3) / (4u² + 3)^(3/2) )

= 2u / (4u² + 3)^(1/2).

Wait, maybe this approach is getting too messy. Alternatively, let's compute the definite integral from u = -1/2 to u = ∞.

But this seems complicated. Maybe there's a better way. Let me recall that I2b is (1/2) times the integral from -1/2 to ∞ of 1/(u² + 3/4)^(5/2) du.

Alternatively, use symmetry. The integrand is even around u = 0 if the limits are symmetric, but here the lower limit is -1/2. Hmm.

Alternatively, use substitution v = u. But not helpful. Alternatively, split the integral into two parts: from -1/2 to 0 and from 0 to ∞.

But this might not help. Alternatively, use the antiderivative we found:

(16/9) [2u/(sqrt(4u² + 3)) - (8u³)/(3(4u² + 3)^(3/2)) ] evaluated from u = -1/2 to u = ∞.

At u = ∞:

First term: 2u / sqrt(4u² + 3) ≈ 2u / (2u) = 1.

Second term: (8u³)/(3(4u² + 3)^(3/2)) ≈ (8u³)/(3*(8u³)) ) = 1/3. So the expression at infinity is 1 - 1/3 = 2/3.

At u = -1/2:

First term: 2*(-1/2)/sqrt(4*(1/4) + 3) = (-1)/sqrt(1 + 3) = (-1)/2.

Second term: (8*(-1/2)^3)/(3*(4*(1/4) + 3)^(3/2)) = (8*(-1/8))/(3*(1 + 3)^(3/2)) = (-1)/(3*(4)^(3/2)) = (-1)/(3*8) = -1/24.

So the expression at u = -1/2 is (-1/2) - (-1/24) = -1/2 + 1/24 = -12/24 + 1/24 = -11/24.

Therefore, the definite integral from -1/2 to ∞ is (2/3) - (-11/24) = 2/3 + 11/24 = 16/24 + 11/24 = 27/24 = 9/8.

But wait, the antiderivative was multiplied by 16/9, so the integral is (16/9)*(9/8) = 2.

Wait, let me check:

The antiderivative evaluated from -1/2 to ∞ is [2/3 - (-11/24)] = 2/3 + 11/24 = (16/24 + 11/24) = 27/24 = 9/8. Then multiply by 16/9:

16/9 * 9/8 = 16/8 = 2. So the integral I2b is (1/2)*2 = 1.

Therefore, I2 = I2a + I2b = 1/3 + 1 = 4/3.

So going back to the original expression:

The integral is 2*(I1 + I2) = 2*(2 + 4/3) = 2*(10/3) = 20/3.

Wait, wait, no. Wait, the original integral was 2*(I1 + I2), where I1 was 2 and I2 was 4/3. Wait, no:

Wait, the original integral after substitution became 2*(I1 + I2), where I1 was ∫₀^∞ 1/(t² - t + 1)^(3/2) dt = 2, and I2 was ∫₀^∞ t/(t² - t + 1)^(5/2) dt = 4/3. So the total integral is 2*(2 + 4/3) = 2*(10/3) = 20/3.

Wait, but 2*(2 + 4/3) = 2*(10/3) = 20/3. So the definite integral evaluates to 20/3.

But let me verify this result. Let me check the steps again to make sure I didn't make a mistake.

First substitution: x = sin²θ, leading to 2 ∫ cosθ [1 - sinθ cosθ]^(-5/2) dθ. Then after various substitutions, we ended up with 20/3. Alternatively, maybe there's a simpler way.

Alternatively, let's check with a substitution in the original integral. Let me consider substituting x = sin²θ. Then, as before, the integral becomes 2 ∫₀^(π/2) cosθ [1 - sinθ cosθ]^(-5/2) dθ. Let me try to compute this integral directly.

Let me set t = sinθ. Then dt = cosθ dθ. The integral becomes 2 ∫₀¹ [1 - t sqrt(1 - t²)]^(-5/2) dt. Let me set u = t sqrt(1 - t²). Then, but this might not help. Alternatively, set u = sinφ. Not sure.

Alternatively, use substitution u = t^2. Hmm, not helpful. Alternatively, note that t sqrt(1 - t²) = (1/2) sin2θ, but θ is already substituted. Hmm.

Alternatively, use a substitution where v = t sqrt(1 - t²). Let me try:

Let v = t sqrt(1 - t²). Then, compute dv/dt:

dv/dt = sqrt(1 - t²) + t*( -2t )/(2 sqrt(1 - t²)) ) = sqrt(1 - t²) - t² / sqrt(1 - t²) = (1 - t² - t²)/sqrt(1 - t²) = (1 - 2t²)/sqrt(1 - t²).

Not sure if helpful. Alternatively, maybe use substitution v = t^2. Then dv = 2t dt. But not sure.

Alternatively, consider that the integral after substitution is 2 ∫₀¹ [1 - t sqrt(1 - t²)]^(-5/2) dt. Let me compute this numerically for a quick check. Let's pick t = 0.5. Then sqrt(1 - t²) = sqrt(3)/2 ≈ 0.866. So 1 - t sqrt(1 - t²) ≈ 1 - 0.5*0.866 ≈ 1 - 0.433 ≈ 0.567. Then [0.567]^(-5/2) ≈ (0.567)^(-2.5) ≈ (1/0.567^2)^(1.25). Wait, maybe approximate:

0.567 is approximately 0.567, so 0.567^2 ≈ 0.321. Then 1/0.321 ≈ 3.115. Then 3.115^1.25 ≈ e^(1.25 ln3.115) ≈ e^(1.25*1.136) ≈ e^(1.42) ≈ 4.14. So the integrand at t=0.5 is approximately 4.14. But integrating from 0 to 1, the integral might be around 20/3 ≈ 6.666... But this is just a rough check. Alternatively, compute the numerical value later.

But according to the previous steps, the integral evaluates to 20/3. Let me check if that makes sense. Let's compute the numerical approximation.

The exact answer is 20/3 ≈ 6.6666666667. Let me verify with a numerical approximation.

But since the user also asks for a numerical approximation, I can compute it numerically. However, since I'm supposed to provide the exact answer first, let's confirm the steps again.

Wait, in the previous steps, after substitution, the integral became 2*(I1 + I2) = 2*(2 + 4/3) = 20/3. So the exact answer is 20/3. Let me check if this is correct.

Alternatively, maybe there's a mistake in the substitution steps. Let me check the substitution where x = t²/(1 + t²). Then dx = 2t/(1 + t²)^2 dt. Then the integral became 2 ∫₀^∞ (1 + t²)/(t² - t + 1)^(5/2) dt. Then splitting into I1 and I2, which were computed as 2 and 4/3, leading to 20/3. That seems correct.

Alternatively, the integral might be expressed in terms of beta functions. Let me see. The original integral is ∫₀¹ x^(-1/2) [1 - sqrt(x(1 - x))]^(-5/2) dx. Let me consider substitution y = sqrt(x(1 - x)). Then y = sqrt(x - x²), y² = x - x², x² - x + y² = 0. Solving for x: x = [1 ± sqrt(1 - 4y²)]/2. But this might not help.

Alternatively, use substitution z = sqrt(x). Let z = sqrt(x), so x = z², dx = 2z dz. Then the integral becomes ∫₀¹ (z²)^(-1/2) [1 - sqrt(z²(1 - z²))]^(-5/2) * 2z dz = 2 ∫₀¹ z^(-1) [1 - z sqrt(1 - z²)]^(-5/2) z dz = 2 ∫₀¹ [1 - z sqrt(1 - z²)]^(-5/2) dz.

Hmm, similar to previous substitutions. Not helpful.

Alternatively, consider that the integral might be related to the beta function. Let me recall that beta function is ∫₀¹ t^{c-1}(1 - t)^{d -c -1} dt. But the integrand here is x^{-1/2} [1 - sqrt(x(1 - x))]^{-5/2}. Not obviously a beta function, but perhaps after substitution.

Alternatively, use substitution u = sqrt(x(1 - x)). Then u² = x(1 - x). Let me solve for x: x(1 - x) = u² => x² - x + u² = 0. The solutions are x = [1 ± sqrt(1 - 4u²)]/2. But this might not help.

Alternatively, use substitution t = x/(1 - x). Then x = t/(1 + t), dx = dt/(1 + t)^2. The integral becomes:

∫₀^∞ [ t/(1 + t) ]^(-1/2) [1 - sqrt( t/(1 + t) * (1 - t/(1 + t)) ) ]^(-5/2) * dt/(1 + t)^2.

Simplify:

First term: [ t/(1 + t) ]^(-1/2) = (1 + t)^(1/2) / t^(1/2).

Inside the brackets: sqrt( t/(1 + t) * (1/(1 + t)) ) = sqrt( t/(1 + t)^2 ) = sqrt(t)/(1 + t).

So the term becomes 1 - sqrt(t)/(1 + t). Therefore, [1 - sqrt(t)/(1 + t)]^(-5/2).

Putting it all together:

∫₀^∞ (1 + t)^(1/2)/t^(1/2) * [1 - sqrt(t)/(1 + t)]^(-5/2) * dt/(1 + t)^2.

Simplify:

(1 + t)^(1/2) / t^(1/2) * 1/(1 + t)^2 = 1/( t^(1/2) (1 + t)^(3/2) ).

So the integral becomes:

∫₀^∞ [1 - sqrt(t)/(1 + t)]^(-5/2) * 1/( t^(1/2) (1 + t)^(3/2) ) dt.

Not sure if this helps. Maybe another substitution. Let me set u = sqrt(t). Then t = u², dt = 2u du. The integral becomes:

∫₀^∞ [1 - u/(1 + u²)]^(-5/2) * 1/( u (1 + u²)^(3/2) ) * 2u du.

Simplify:

2 ∫₀^∞ [1 - u/(1 + u²)]^(-5/2) * 1/( (1 + u²)^(3/2) ) du.

The term inside the brackets: 1 - u/(1 + u²) = (1 + u² - u)/(1 + u²).

So the integral becomes:

2 ∫₀^∞ [ (1 + u² - u)/(1 + u²) ]^(-5/2) * 1/(1 + u²)^(3/2) du.

Simplify the exponents:

[ (1 + u² - u)/(1 + u²) ]^(-5/2) = (1 + u²)^(5/2) / (1 + u² - u)^(5/2).

Therefore, the integral is:

2 ∫₀^∞ (1 + u²)^(5/2) / (1 + u² - u)^(5/2) * 1/(1 + u²)^(3/2) du = 2 ∫₀^∞ (1 + u²)^(5/2 - 3/2) / (1 + u² - u)^(5/2) du = 2 ∫₀^∞ (1 + u²) / (1 + u² - u)^(5/2) du.

This is the same integral as before, which we evaluated to 20/3. So this confirms that the integral is indeed 20/3.

Therefore, the exact answer is 20/3. The numerical approximation is approximately 6.6666666667. Rounded to 10 decimal places, that's 6.6666666667.

So the final answer is {"answer": "\\dfrac{20}{3}", "numerical_answer": 6.6666666667}.
</think>

{"answer": "\\dfrac{20}{3}", "numerical_answer": 6.6666666667}