

To solve the definite integral 

\[
\int_{0}^{2} \frac{x^{-1/2}(2-x)^{-1/2}}{\sqrt{1 + x(2 - x)}} T_3\left(\sqrt{1 + x(2 - x)}\right) \, dx,
\]

we proceed as follows:

### Step 1: Simplify the integrand using Chebyshev polynomials
The third Chebyshev polynomial of the first kind is \( T_3(t) = 4t^3 - 3t \). Let \( u = \sqrt{1 + x(2 - x)} \), so \( T_3(u) = 4u^3 - 3u \). Substituting this into the integrand, we get:
\[
\frac{x^{-1/2}(2-x)^{-1/2}}{\sqrt{1 + x(2 - x)}} \cdot (4u^3 - 3u).
\]
Since \( u = \sqrt{1 + x(2 - x)} \), the denominator \( \sqrt{1 + x(2 - x)} = u \), so the integrand simplifies to:
\[
x^{-1/2}(2-x)^{-1/2} \cdot (4u^2 - 3).
\]

### Step 2: Substitution to simplify the domain
Let \( t = x - 1 \), so \( x = t + 1 \) and \( 2 - x = 1 - t \). When \( x \in [0, 2] \), \( t \in [-1, 1] \). The term \( x(2 - x) \) becomes \( (t + 1)(1 - t) = 1 - t^2 \), so \( u^2 = 1 + (1 - t^2) = 2 - t^2 \). Thus, \( 4u^2 - 3 = 4(2 - t^2) - 3 = 5 - 4t^2 \).

The term \( x^{-1/2}(2 - x)^{-1/2} \) becomes \( [(t + 1)(1 - t)]^{-1/2} = (1 - t^2)^{-1/2} \). The integral now transforms to:
\[
\int_{-1}^{1} \frac{5 - 4t^2}{\sqrt{1 - t^2}} \, dt.
\]

### Step 3: Evaluate the simplified integral
Split the integral into two parts:
\[
5 \int_{-1}^{1} \frac{1}{\sqrt{1 - t^2}} \, dt - 4 \int_{-1}^{1} \frac{t^2}{\sqrt{1 - t^2}} \, dt.
\]

- The first integral is \( \int_{-1}^{1} \frac{1}{\sqrt{1 - t^2}} \, dt = \pi \) (since it is the integral of the derivative of \( \arcsin(t) \) over its full domain).
- The second integral uses the substitution \( t = \sin\theta \), leading to \( \int_{-1}^{1} \frac{t^2}{\sqrt{1 - t^2}} \, dt = \frac{\pi}{2} \).

Thus, the integral evaluates to:
\[
5\pi - 4 \cdot \frac{\pi}{2} = 5\pi - 2\pi = 3\pi.
\]

### Numerical Approximation
The numerical value of \( 3\pi \) is approximately \( 9.4247779608 \) (rounded to 10 decimal places).

{"answer": "3\pi", "numerical_answer": "9.4247779608"}