# Evaluating $\int_{0}^{2} x^{-1/2} (2-x)^{-1/2} [1-0.5x(2-x)]^{1} dx$

## Step 1: Analyze the integral
Let's examine the integrand:
$x^{-1/2} (2-x)^{-1/2} [1-0.5x(2-x)]^{1}$

## Step 2: Substitution
Let's use the substitution $x = 2\sin^2(\theta)$. This implies:
- $dx = 4\sin(\theta)\cos(\theta)d\theta$
- When $x = 0$, $\theta = 0$
- When $x = 2$, $\theta = \frac{\pi}{2}$
- $2-x = 2-2\sin^2(\theta) = 2\cos^2(\theta)$

## Step 3: Rewrite the integrand
Let's substitute these values:

$x^{-1/2} = (2\sin^2(\theta))^{-1/2} = \frac{1}{\sqrt{2}\sin(\theta)}$

$(2-x)^{-1/2} = (2\cos^2(\theta))^{-1/2} = \frac{1}{\sqrt{2}\cos(\theta)}$

$1-0.5x(2-x) = 1-0.5(2\sin^2(\theta))(2\cos^2(\theta)) = 1-2\sin^2(\theta)\cos^2(\theta)$

$= 1-\frac{1}{2}\sin^2(2\theta) = 1-\frac{1-\cos(4\theta)}{4} = \frac{3+\cos(4\theta)}{4}$

## Step 4: Putting it all together
Now our integral becomes:
$\int_{0}^{\frac{\pi}{2}} \frac{1}{\sqrt{2}\sin(\theta)} \cdot \frac{1}{\sqrt{2}\cos(\theta)} \cdot \frac{3+\cos(4\theta)}{4} \cdot 4\sin(\theta)\cos(\theta)d\theta$

Simplifying:
$\int_{0}^{\frac{\pi}{2}} \frac{3+\cos(4\theta)}{2} d\theta$

$= \frac{1}{2}\int_{0}^{\frac{\pi}{2}} 3 d\theta + \frac{1}{2}\int_{0}^{\frac{\pi}{2}} \cos(4\theta) d\theta$

$= \frac{3\theta}{2}\bigg|_{0}^{\frac{\pi}{2}} + \frac{1}{8}\sin(4\theta)\bigg|_{0}^{\frac{\pi}{2}}$

$= \frac{3\pi}{4} + \frac{1}{8}\sin(2\pi) - \frac{1}{8}\sin(0)$

$= \frac{3\pi}{4} + 0 = \frac{3\pi}{4}$

## Step 5: Numerical approximation
$\frac{3\pi}{4} â‰ˆ 2.3561944902$

{"answer": "\\frac{3\\pi}{4}", "numerical_answer": "2.3561944902"}