<think>
Okay, so I need to compute the definite integral of ln(x)/(x² + 3) from 1 to 3. Hmm, let's see. I remember that integrals involving logarithms and rational functions can sometimes be tricky. Maybe substitution or integration by parts? Let me think.

First, let me write down the integral again: ∫₁³ [ln(x)/(x² + 3)] dx. The denominator is x squared plus 3, which doesn't factor nicely over the reals. So substitution might not be straightforward here. Integration by parts is another approach. Let me recall the formula: ∫u dv = uv - ∫v du.

Let me set u = ln(x), so du = (1/x) dx. Then dv would be 1/(x² + 3) dx. To find v, I need to integrate dv. The integral of 1/(x² + a²) dx is (1/a) arctan(x/a) + C. So here, a is sqrt(3), so v = (1/sqrt(3)) arctan(x/sqrt(3)).

Applying integration by parts: uv - ∫v du. So that's ln(x)*(1/sqrt(3)) arctan(x/sqrt(3)) evaluated from 1 to 3 minus the integral from 1 to 3 of (1/sqrt(3)) arctan(x/sqrt(3)) * (1/x) dx.

Hmm, so now the remaining integral is (1/sqrt(3)) ∫ [arctan(x/sqrt(3)) / x] dx. This still looks complicated. Maybe another substitution here? Let me think. Let’s set t = x/sqrt(3), so x = t sqrt(3), dx = sqrt(3) dt. Then, substituting, the integral becomes (1/sqrt(3)) ∫ [arctan(t) / (t sqrt(3))] * sqrt(3) dt. The sqrt(3) cancels out, so we have (1/sqrt(3)) * ∫ arctan(t)/t dt.

So now the integral simplifies to (1/sqrt(3)) ∫ arctan(t)/t dt. Hmm, but how do I integrate arctan(t)/t? That doesn't look like a standard integral. Maybe another integration by parts? Let me try. Let’s set u = arctan(t), dv = (1/t) dt. Then du = (1/(1 + t²)) dt, and v = ln|t|. So integration by parts gives arctan(t) ln|t| - ∫ ln|t| * (1/(1 + t²)) dt. But this seems even more complicated. The new integral is ∫ [ln(t)/(1 + t²)] dt, which is similar to the original integral but in terms of t. Wait, but maybe there's a different approach here.

Alternatively, perhaps expanding arctan(t) as a power series? Let me recall that arctan(t) = ∑_{n=0}^∞ (-1)^n t^{2n+1}/(2n+1) for |t| ≤ 1. But here, t = x/sqrt(3), and x ranges from 1 to 3, so t ranges from 1/sqrt(3) to 3/sqrt(3) = sqrt(3). Since sqrt(3) is approximately 1.732, which is greater than 1, so the radius of convergence is 1, which is exceeded here. So the power series might not converge over the entire interval. Hmm, that might not work.

Alternatively, maybe substitution. Let’s consider the integral ∫ arctan(t)/t dt. Let me set u = arctan(t), then du = dt/(1 + t²). But I don't see an obvious substitution here. Alternatively, maybe express arctan(t) as an integral. Wait, arctan(t) = ∫₀^t 1/(1 + s²) ds. So then, ∫ arctan(t)/t dt = ∫ [∫₀^t 1/(1 + s²) ds] / t dt. Maybe switch the order of integration? But that's a double integral. Let me see. Let’s consider integrating over s from 0 to t, and t from some lower limit to upper. But I'm not sure if that helps. Alternatively, differentiation under the integral sign? Maybe not.

Wait, perhaps there's a known integral formula for ∫ arctan(t)/t dt. Let me check. I don't recall one off the top of my head. Maybe look it up? But since I can't actually look things up, I need to think. Let me try substitution. Let’s set z = t². Then dz = 2t dt. Hmm, not sure. Alternatively, set u = ln(t), but that might not help. Wait, maybe integrating by parts again. Let me try that. Let’s set u = arctan(t), dv = (1/t) dt. Then du = (1/(1 + t²)) dt, and v = ln t. So as before, we have arctan(t) ln t - ∫ (ln t)/(1 + t²) dt. But this brings us back to an integral similar to the original problem. Wait, but in terms of t. Let me denote this integral as J = ∫ (ln t)/(1 + t²) dt. If I can express J in terms of the original integral, maybe we can solve for it.

But the original integral was in terms of x, but after substitution, we have t = x/sqrt(3). Let me see. Let's recap. The original integral after substitution became:

After first integration by parts, we had:

[ln(x) * (1/sqrt(3)) arctan(x/sqrt(3))] from 1 to 3 - (1/sqrt(3)) ∫ [arctan(t)/t] dt, where t = x/sqrt(3). Then, when we tried integrating arctan(t)/t, we ended up with J = ∫ (ln t)/(1 + t²) dt. Wait, but the original integral was ∫ [ln x / (x² + 3)] dx. If we make substitution in the original integral, say x = sqrt(3) t, then dx = sqrt(3) dt, and the integral becomes ∫ [ln(sqrt(3) t) / (3 t² + 3)] * sqrt(3) dt = (sqrt(3)/3) ∫ [ln(sqrt(3)) + ln t] / (t² + 1) dt. Which splits into two terms: (sqrt(3)/3) ln(sqrt(3)) ∫ 1/(t² +1) dt + (sqrt(3)/3) ∫ (ln t)/(t² +1) dt. The first integral is (sqrt(3)/3) ln(sqrt(3)) * arctan(t) + ... and the second integral is (sqrt(3)/3) J, where J is the same as before. But this seems like a different approach. Maybe this substitution can help relate the original integral to J?

Wait, but in the original problem, after integration by parts, we have an expression involving J. So perhaps if we can express J in terms of the original integral, we can set up an equation and solve for the original integral. Let me try to formalize this.

Let’s denote the original integral as I = ∫₁³ [ln x / (x² + 3)] dx.

After integration by parts, we have:

I = [ln x * (1/sqrt(3)) arctan(x/sqrt(3))] from 1 to 3 - (1/sqrt(3)) ∫₁³ [arctan(x/sqrt(3)) / x] dx.

Let’s call the remaining integral K = ∫₁³ [arctan(x/sqrt(3)) / x] dx.

So, I = (1/sqrt(3)) [ln(3) arctan(3/sqrt(3)) - ln(1) arctan(1/sqrt(3))] - (1/sqrt(3)) K.

Since ln(1) is 0, this simplifies to:

I = (1/sqrt(3)) ln(3) arctan(sqrt(3)) - (1/sqrt(3)) K.

Now, arctan(sqrt(3)) is π/3, since tan(π/3) = sqrt(3). So:

I = (1/sqrt(3)) ln(3) * (π/3) - (1/sqrt(3)) K.

So, I = (π ln 3)/(3 sqrt(3)) - (1/sqrt(3)) K.

Now, we need to compute K = ∫₁³ [arctan(x/sqrt(3)) / x] dx.

Let’s make substitution t = x/sqrt(3), so x = t sqrt(3), dx = sqrt(3) dt. Then, when x=1, t=1/sqrt(3), and x=3, t=3/sqrt(3)=sqrt(3). So K becomes:

K = ∫_{1/sqrt(3)}^{sqrt(3)} [arctan(t) / (t sqrt(3))] * sqrt(3) dt = ∫_{1/sqrt(3)}^{sqrt(3)} [arctan(t)/t] dt.

So K = ∫_{a}^{b} [arctan(t)/t] dt, where a =1/sqrt(3), b=sqrt(3).

Now, when we tried integrating arctan(t)/t earlier, we ended up with an expression involving J = ∫ [ln t / (1 + t²)] dt. Let me recall that:

∫ arctan(t)/t dt = arctan(t) ln t - ∫ [ln t / (1 + t²)] dt.

So, K = [arctan(t) ln t] from a to b - ∫_{a}^{b} [ln t / (1 + t²)] dt.

Let’s compute this:

First term: [arctan(b) ln b - arctan(a) ln a].

Second term: - ∫_{a}^{b} [ln t / (1 + t²)] dt.

But notice that the integral ∫ [ln t / (1 + t²)] dt is similar to the original integral I, but with different limits and variable. Let me see. Let’s denote this integral as J = ∫ [ln t / (1 + t²)] dt. If we can relate J to I, maybe we can express K in terms of I.

But in the original substitution, when we set x = sqrt(3) t, the original integral I becomes:

I = ∫₁³ [ln x / (x² + 3)] dx = ∫_{1/sqrt(3)}^{sqrt(3)} [ln(sqrt(3) t) / (3 t² + 3)] * sqrt(3) dt.

Simplify:

= (sqrt(3)/3) ∫_{a}^{b} [ln(sqrt(3)) + ln t] / (t² +1) dt.

= (sqrt(3)/3) ln(sqrt(3)) ∫_{a}^{b} 1/(t² +1) dt + (sqrt(3)/3) ∫_{a}^{b} [ln t)/(t² +1)] dt.

The first term is (sqrt(3)/3) ln(sqrt(3)) [arctan(b) - arctan(a)].

The second term is (sqrt(3)/3) J, where J is the integral from a to b of [ln t / (t² +1)] dt.

But notice that J is exactly the same as the integral in the expression for K. So, from the expression for K:

K = [arctan(b) ln b - arctan(a) ln a] - J.

So, J = [arctan(b) ln b - arctan(a) ln a] - K.

But from the expression for I in terms of J:

I = (sqrt(3)/3) ln(sqrt(3)) [arctan(b) - arctan(a)] + (sqrt(3)/3) J.

Substituting J from above:

I = (sqrt(3)/3) ln(sqrt(3)) [arctan(b) - arctan(a)] + (sqrt(3)/3) [ [arctan(b) ln b - arctan(a) ln a] - K ].

But we also have from earlier expression:

I = (π ln 3)/(3 sqrt(3)) - (1/sqrt(3)) K.

So now we have two expressions for I. Let me write them down:

First expression:

I = (π ln 3)/(3 sqrt(3)) - (1/sqrt(3)) K.

Second expression:

I = (sqrt(3)/3) ln(sqrt(3)) [arctan(b) - arctan(a)] + (sqrt(3)/3) [ arctan(b) ln b - arctan(a) ln a - K ].

Let me substitute the values of a and b. Remember a =1/sqrt(3), b=sqrt(3).

First, compute arctan(b) = arctan(sqrt(3)) = π/3.

arctan(a) = arctan(1/sqrt(3)) = π/6.

Also, ln(sqrt(3)) = (1/2) ln 3.

So, let's compute the second expression:

First term: (sqrt(3)/3) * (1/2 ln 3) * [π/3 - π/6] = (sqrt(3)/3)( (ln 3)/2 )( π/6 ) = (sqrt(3) ln 3 π)/36.

Second term: (sqrt(3)/3) [ (π/3) ln(sqrt(3)) - (π/6) ln(1/sqrt(3)) - K ].

Compute ln(sqrt(3)) = (1/2) ln 3, ln(1/sqrt(3)) = - (1/2) ln 3.

So:

(π/3)(1/2 ln 3) - (π/6)(-1/2 ln 3) = (π ln 3)/6 + (π ln 3)/12 = (2π ln 3 + π ln 3)/12 = (3π ln 3)/12 = (π ln 3)/4.

Therefore, the second term becomes (sqrt(3)/3) [ (π ln 3)/4 - K ].

Putting it all together, the second expression for I is:

I = (sqrt(3) ln 3 π)/36 + (sqrt(3)/3)( (π ln 3)/4 - K )

= (sqrt(3) π ln 3)/36 + (sqrt(3) π ln 3)/(12) - (sqrt(3)/3) K.

Combine the terms:

First term: sqrt(3) π ln 3 /36

Second term: sqrt(3) π ln 3 /12 = 3 sqrt(3) π ln 3 /36

So total: (1 + 3)/36 sqrt(3) π ln 3 = 4/36 sqrt(3) π ln 3 = sqrt(3) π ln 3 /9.

Thus, the second expression is:

I = sqrt(3) π ln 3 /9 - (sqrt(3)/3) K.

But from the first expression, I = (π ln 3)/(3 sqrt(3)) - (1/sqrt(3)) K.

Let me write both expressions:

First: I = (π ln 3)/(3 sqrt(3)) - (1/sqrt(3)) K.

Second: I = sqrt(3) π ln 3 /9 - (sqrt(3)/3) K.

Let me check if these are equivalent. Let's compute (π ln 3)/(3 sqrt(3)):

Multiply numerator and denominator by sqrt(3): (π ln 3 sqrt(3))/(3*3) = sqrt(3) π ln 3 /9. So yes, the first term of the same as the second expression. Similarly, -(1/sqrt(3)) K is the same as - (sqrt(3)/3) K * (3/sqrt(3))? Wait, no. Wait, the coefficients:

First expression: - (1/sqrt(3)) K.

Second expression: - (sqrt(3)/3) K.

But sqrt(3)/3 = 1/sqrt(3). Because sqrt(3)/3 = (sqrt(3)/sqrt(3)^2) = 1/sqrt(3). So yes, both expressions are the same. So this doesn't help us solve for K. Hmm, so this approach leads us in circles.

Hmm, so maybe there's another way. Let me think. Perhaps consider substitution t = 1/u in the integral K. Let’s try that. Let’s set t = 1/u, so when t = a =1/sqrt(3), u = sqrt(3), and when t = b = sqrt(3), u =1/sqrt(3). Then dt = -1/u² du. So K becomes:

K = ∫_{sqrt(3)}^{1/sqrt(3)} [arctan(1/u) / (1/u)] * (-1/u²) du.

Simplify:

= ∫_{1/sqrt(3)}^{sqrt(3)} [arctan(1/u) * u] * (1/u²) du.

= ∫_{1/sqrt(3)}^{sqrt(3)} [arctan(1/u) / u] du.

But arctan(1/u) = π/2 - arctan(u) for u >0. So:

K = ∫_{1/sqrt(3)}^{sqrt(3)} [ (π/2 - arctan(u)) / u ] du.

= (π/2) ∫_{1/sqrt(3)}^{sqrt(3)} (1/u) du - ∫_{1/sqrt(3)}^{sqrt(3)} [arctan(u)/u] du.

The first integral is (π/2) [ln u] from 1/sqrt(3) to sqrt(3)} = (π/2)(ln sqrt(3) - ln(1/sqrt(3))) = (π/2)( (1/2 ln 3) - (-1/2 ln 3) ) = (π/2)( ln 3 ) = (π ln 3)/2.

The second integral is exactly K. So:

K = (π ln 3)/2 - K.

So, K + K = (π ln 3)/2 => 2K = (π ln 3)/2 => K = (π ln 3)/4.

Oh! That's a clever substitution. So K = (π ln 3)/4.

Now, going back to the expression for I:

I = (π ln 3)/(3 sqrt(3)) - (1/sqrt(3)) K.

Substituting K:

I = (π ln 3)/(3 sqrt(3)) - (1/sqrt(3))*(π ln 3)/4.

Factor out (π ln 3)/sqrt(3):

I = (π ln 3)/sqrt(3) [1/3 - 1/4] = (π ln 3)/sqrt(3) * (1/12) * (4 - 3) = (π ln 3)/sqrt(3) * (1/12) *1 = (π ln 3)/(12 sqrt(3)).

Wait, wait, let me compute [1/3 - 1/4] = (4 - 3)/12 = 1/12. So:

I = (π ln 3)/sqrt(3) * (1/12) = (π ln 3)/(12 sqrt(3)).

But we can rationalize the denominator:

Multiply numerator and denominator by sqrt(3):

= (π ln 3 sqrt(3))/(12 * 3) = (π ln 3 sqrt(3))/36.

Alternatively, leave it as (π ln 3)/(12 sqrt(3)).

But both are correct. However, typically, we might prefer to rationalize the denominator. So:

I = (π ln 3 sqrt(3))/36.

Alternatively, written as (sqrt(3) π ln 3)/36.

But let me check the steps again to make sure.

We had K = (π ln 3)/4.

Then I = (π ln 3)/(3 sqrt(3)) - (1/sqrt(3))*(π ln 3)/4.

Compute each term:

First term: (π ln 3)/(3 sqrt(3)).

Second term: (π ln 3)/(4 sqrt(3)).

So I = (π ln 3)/(3 sqrt(3)) - (π ln 3)/(4 sqrt(3)) = (π ln 3)/sqrt(3) [1/3 - 1/4] = (π ln 3)/sqrt(3) * (1/12) = (π ln 3)/(12 sqrt(3)).

Yes, that's correct. So the exact answer is π ln 3 divided by (12 sqrt(3)).

Alternatively, combining the constants:

sqrt(3)/12 = 1/(4 sqrt(3)), but perhaps it's better to rationalize:

Multiply numerator and denominator by sqrt(3):

(π ln 3 * sqrt(3)) / (12 * 3) = (π ln 3 sqrt(3))/36.

So, both forms are acceptable. Let me check which is more standard. Probably the rationalized form. So the exact answer is (π ln 3 sqrt(3))/36.

Alternatively, written as (sqrt(3) π ln 3)/36.

Either way, both are correct. Let me confirm the steps once more to ensure no mistakes.

1. Integration by parts: correct.

2. Substitution t = x/sqrt(3): correct.

3. Recognizing that K can be expressed via substitution t =1/u and using arctan(1/u) = π/2 - arctan(u): correct.

4. Solving for K: yes, leading to K = (π ln 3)/4.

5. Substituting back into I: correct, leading to I = (π ln 3)/(12 sqrt(3)).

Yes, this seems correct.

Now, for the numerical approximation. Let's compute this value.

First, compute the exact expression:

I = (π * ln 3 * sqrt(3)) / 36.

Compute each constant:

π ≈ 3.1415926536

ln 3 ≈ 1.0986122887

sqrt(3) ≈ 1.7320508076

Multiply them together:

π * ln 3 ≈ 3.1415926536 * 1.0986122887 ≈ 3.1415926536 * 1.0986122887 ≈ Let's compute:

3 * 1.0986 = 3.2958

0.1415926536 * 1.0986 ≈ 0.1415926536 *1 =0.1415926536, 0.1415926536*0.0986≈0.01396. So total ≈0.1415926536 +0.01396≈0.15555. So total π*ln3≈3.2958 +0.15555≈3.45135.

Then multiply by sqrt(3) ≈1.7320508076:

3.45135 *1.7320508076 ≈

3 *1.73205=5.19615

0.45135*1.73205≈0.45135*1.7≈0.7673, 0.45135*0.03205≈0.01447. Total≈0.7673+0.01447≈0.78177.

Total ≈5.19615 +0.78177≈5.97792.

Then divide by 36:

5.97792 /36 ≈0.166053.

So approximately 0.166053. Let me check with a calculator for more precision.

Alternatively, use more accurate values:

Compute π ≈3.141592653589793

ln3≈1.0986122886681098

sqrt(3)≈1.7320508075688772

Multiply all three:

3.141592653589793 *1.0986122886681098 = let's compute:

3.141592653589793 *1 =3.141592653589793

3.141592653589793 *0.0986122886681098≈

First, 3.141592653589793 *0.1=0.3141592653589793

Subtract 3.141592653589793 *0.0013877113318902≈

3.141592653589793 *0.001=0.003141592653589793

3.141592653589793 *0.0003877113318902≈approx 0.0003877*3.14159≈0.001217

So total subtract: 0.00314159 +0.001217≈0.0043586

So 0.3141592653589793 -0.0043586≈0.3098006

So total π*ln3≈3.141592653589793 +0.3098006≈3.45139325

Now multiply by sqrt(3)=1.7320508075688772:

3.45139325 *1.7320508075688772

Compute 3 *1.73205=5.19615

0.45139325 *1.73205≈

0.4*1.73205=0.69282

0.05139325*1.73205≈0.05139325*1.7≈0.087368, 0.05139325*0.03205≈0.001647

Total≈0.69282 +0.087368 +0.001647≈0.781835

So total≈5.19615 +0.781835≈5.977985

Divide by 36:5.977985 /36≈0.1660551389.

So approximately 0.1660551389. Rounded to 10 decimal places, that's 0.1660551390.

But let me check using a calculator for more precision.

Alternatively, use a calculator:

Compute (π * ln(3) * sqrt(3)) / 36.

Using a calculator:

π ≈3.141592653589793

ln(3)≈1.0986122886681098

sqrt(3)≈1.7320508075688772

Multiply them: 3.141592653589793 *1.0986122886681098 = 3.451393269700642

Then multiply by 1.7320508075688772: 3.451393269700642 *1.7320508075688772 ≈5.977985463260682

Divide by 36:5.977985463260682 /36 ≈0.16605515175724117.

So approximately 0.1660551518, which rounds to 0.1660551518, so to 10 decimal places: 0.1660551518.

But let me verify with another method. Alternatively, compute the integral numerically using substitution.

Alternatively, use numerical integration methods like Simpson's rule, but since this is supposed to be a numerical approximation, perhaps use a calculator.

But given that the exact value is (π ln3 sqrt(3))/36 ≈0.1660551518, so the numerical approximation is approximately 0.1660551518, which rounds to 0.1660551518, so to 10 decimal places: 0.1660551518.

But let me check with another approach. Let's compute the integral numerically using substitution.

Alternatively, use substitution x = sqrt(3) tanθ, but maybe not necessary. Alternatively, use a calculator.

But since we already have the exact expression, and the numerical value is approximately 0.1660551518, which is about 0.1660551518.

So the final answer is:

Exact: (sqrt(3) π ln 3)/36

Numerical: approximately 0.1660551518.

So the JSON output should be:

{"answer": "\\frac{\\sqrt{3} \\pi \\ln(3)}{36}", "numerical_answer": "0.1660551518"}

Let me check the LaTeX for the exact answer: \frac{\sqrt{3} \pi \ln(3)}{36}. Yes, that's correct.
</think>

{"answer": "\\frac{\\sqrt{3} \\pi \\ln(3)}{36}", "numerical_answer": "0.1660551518"}