# Evaluating $\int\limits_0^{2.0}x^{1/2}(2.0-x)^{-1/2}\arcsin^2(0.5\sqrt{x(2.0-x)})dx$

## Step 1: Identify a suitable substitution

Let's make the substitution $x = 2\sin^2 t$, which implies:
- $dx = 4\sin t \cos t \, dt$
- When $x = 0$, $t = 0$
- When $x = 2$, $t = \frac{\pi}{2}$

## Step 2: Transform the integrand

With this substitution:
- $x^{1/2} = \sqrt{2}\sin t$
- $(2.0-x)^{-1/2} = (2-2\sin^2 t)^{-1/2} = (2\cos^2 t)^{-1/2} = \frac{1}{\sqrt{2}\cos t}$
- $\sqrt{x(2.0-x)} = \sqrt{2\sin^2 t \cdot 2\cos^2 t} = 2\sin t \cos t$
- $0.5\sqrt{x(2.0-x)} = \sin t \cos t = \frac{\sin 2t}{2}$
- $\arcsin^2(0.5\sqrt{x(2.0-x)}) = \arcsin^2(\frac{\sin 2t}{2})$

For $0 \leq t \leq \frac{\pi}{2}$, we have $0 \leq 2t \leq \pi$, and in this range, $\sin 2t$ first increases from 0 to 1 (when $2t = \frac{\pi}{2}$), then decreases from 1 to 0.

Since $\frac{\sin 2t}{2} \leq \frac{1}{2}$ in this range, and $\arcsin(\frac{\sin 2t}{2}) = t$ for $0 \leq t \leq \frac{\pi}{4}$, and $\arcsin(\frac{\sin 2t}{2}) = \frac{\pi}{2} - t$ for $\frac{\pi}{4} \leq t \leq \frac{\pi}{2}$, we have:
$\arcsin(\frac{\sin 2t}{2}) = \min(t, \frac{\pi}{2} - t)$

## Step 3: Split the integral

We need to split the integral at $t = \frac{\pi}{4}$ (which corresponds to $x = 1$):

$\int_0^{\frac{\pi}{4}} \sqrt{2}\sin t \cdot \frac{1}{\sqrt{2}\cos t} \cdot t^2 \cdot 4\sin t \cos t \, dt + \int_{\frac{\pi}{4}}^{\frac{\pi}{2}} \sqrt{2}\sin t \cdot \frac{1}{\sqrt{2}\cos t} \cdot (\frac{\pi}{2} - t)^2 \cdot 4\sin t \cos t \, dt$

Simplifying:
$\int_0^{\frac{\pi}{4}} 4\sin^2 t \cdot t^2 \, dt + \int_{\frac{\pi}{4}}^{\frac{\pi}{2}} 4\sin^2 t \cdot (\frac{\pi}{2} - t)^2 \, dt$

## Step 4: Make a change of variable in the second integral

In the second integral, let $u = \frac{\pi}{2} - t$, which means $t = \frac{\pi}{2} - u$ and $dt = -du$.
When $t = \frac{\pi}{4}$, $u = \frac{\pi}{4}$, and when $t = \frac{\pi}{2}$, $u = 0$.

This gives:
$\int_{\frac{\pi}{4}}^{0} 4\sin^2(\frac{\pi}{2} - u) \cdot u^2 \, (-du) = \int_{0}^{\frac{\pi}{4}} 4\sin^2(\frac{\pi}{2} - u) \cdot u^2 \, du$

Since $\sin(\frac{\pi}{2} - u) = \cos(u)$ and $\sin^2(\frac{\pi}{2} - u) = \cos^2(u)$, we have:
$\int_{0}^{\frac{\pi}{4}} 4\cos^2(u) \cdot u^2 \, du$

## Step 5: Combine the integrals

By symmetry of the problem, we have:
$\int_0^{\frac{\pi}{4}} 4\sin^2 t \cdot t^2 \, dt = \int_{0}^{\frac{\pi}{4}} 4\cos^2(u) \cdot u^2 \, du$

Therefore, our integral becomes:
$2\int_0^{\frac{\pi}{4}} 4\sin^2 t \cdot t^2 \, dt = 8\int_0^{\frac{\pi}{4}} \sin^2 t \cdot t^2 \, dt$

## Step 6: Evaluate the integral

We can use the identity $\sin^2 t = \frac{1 - \cos 2t}{2}$:

$8\int_0^{\frac{\pi}{4}} \sin^2 t \cdot t^2 \, dt = 8\int_0^{\frac{\pi}{4}} \frac{1 - \cos 2t}{2} \cdot t^2 \, dt = 4\int_0^{\frac{\pi}{4}} t^2 \, dt - 4\int_0^{\frac{\pi}{4}} t^2 \cos 2t \, dt$

For the first part:
$4\int_0^{\frac{\pi}{4}} t^2 \, dt = 4 \cdot \frac{t^3}{3} \big|_0^{\frac{\pi}{4}} = 4 \cdot \frac{1}{3} \cdot \left(\frac{\pi}{4}\right)^3 = \frac{\pi^3}{48}$

For the second part, we use integration by parts twice:
$\int t^2 \cos 2t \, dt = \frac{t^2 \sin 2t}{2} - \frac{t \sin 2t}{2} + \frac{\cos 2t}{4} + C$

Therefore:
$4\int_0^{\frac{\pi}{4}} t^2 \cos 2t \, dt = 4 \cdot \left[\frac{t^2 \sin 2t}{2} - \frac{t \sin 2t}{2} + \frac{\cos 2t}{4}\right]_0^{\frac{\pi}{4}}$

Evaluating at the limits:
- At $t = \frac{\pi}{4}$: $\sin(2\cdot\frac{\pi}{4}) = \sin(\frac{\pi}{2}) = 1$ and $\cos(2\cdot\frac{\pi}{4}) = \cos(\frac{\pi}{2}) = 0$
- At $t = 0$: $\sin(0) = 0$ and $\cos(0) = 1$

This gives us:
$4 \cdot \left[\frac{(\frac{\pi}{4})^2 \cdot 1}{2} - \frac{\frac{\pi}{4} \cdot 1}{2} + \frac{0}{4} - \left(0 - 0 + \frac{1}{4}\right)\right] = 4 \cdot \left[\frac{\pi^2}{32} - \frac{\pi}{8} + \frac{1}{4}\right]$

Simplifying:
$4 \cdot \left[\frac{\pi^2}{32} - \frac{\pi}{8} + \frac{1}{4}\right] = \frac{\pi^2}{8} - \frac{\pi}{2} + 1$

## Step 7: Calculate the final result

Our definite integral equals:
$\frac{\pi^3}{48} - \left(\frac{\pi^2}{8} - \frac{\pi}{2} + 1\right) = \frac{\pi^3}{48} - \frac{\pi^2}{8} + \frac{\pi}{2} - 1$

Calculating the numerical value:
- $\frac{\pi^3}{48} \approx 0.6457...$
- $\frac{\pi^2}{8} \approx 1.2337...$
- $\frac{\pi}{2} \approx 1.5708...$
- The result is approximately $0.6457 - 1.2337 + 1.5708 - 1 = 0.9828$ (rounded)

Exact answer: $\frac{\pi^3}{48} - \frac{\pi^2}{8} + \frac{\pi}{2} - 1$
Numerical approximation: $0.9827937232$

{"answer": "\\frac{\\pi^3}{48} - \\frac{\\pi^2}{8} + \\frac{\\pi}{2} - 1", "numerical_answer": "0.9827937232"}