Let's compute the definite integral step by step:

\[
\int_0^1 \left(e^{e^x} - e^{e^x - x}\right) \, dx
\]

### Step 1: Split the Integral
First, split the integral into two parts:

\[
\int_0^1 e^{e^x} \, dx - \int_0^1 e^{e^x - x} \, dx
\]

### Step 2: Simplify the Second Integral
Let's focus on the second integral:

\[
\int_0^1 e^{e^x - x} \, dx
\]

Make the substitution \( u = e^x \). Then, \( du = e^x \, dx \), so \( dx = \frac{du}{u} \). The limits change as follows:
- When \( x = 0 \), \( u = 1 \).
- When \( x = 1 \), \( u = e \).

Substituting into the integral:

\[
\int_0^1 e^{e^x - x} \, dx = \int_1^e e^{u} \cdot e^{-\ln u} \cdot \frac{du}{u}
\]

Simplify the integrand:

\[
e^{u} \cdot e^{-\ln u} \cdot \frac{1}{u} = e^{u} \cdot \frac{1}{u} \cdot \frac{1}{u} = \frac{e^{u}}{u^2}
\]

Thus, the integral becomes:

\[
\int_1^e \frac{e^{u}}{u^2} \, du
\]

### Step 3: Integrate by Parts
Integrate \( \int \frac{e^{u}}{u^2} \, du \) by parts. Let:
- \( v = e^{u} \), so \( dv = e^{u} \, du \).
- \( dw = \frac{1}{u^2} \, du \), so \( w = -\frac{1}{u} \).

Applying integration by parts:

\[
\int \frac{e^{u}}{u^2} \, du = -\frac{e^{u}}{u} + \int \frac{e^{u}}{u} \, du
\]

The remaining integral \( \int \frac{e^{u}}{u} \, du \) is the exponential integral \( \text{Ei}(u) \). Thus:

\[
\int \frac{e^{u}}{u^2} \, du = -\frac{e^{u}}{u} + \text{Ei}(u) + C
\]

Evaluate from \( 1 \) to \( e \):

\[
\left[ -\frac{e^{u}}{u} + \text{Ei}(u) \right]_1^e = -\frac{e^{e}}{e} + \text{Ei}(e) + \frac{e^{1}}{1} - \text{Ei}(1)
\]

Simplify:

\[
- e^{e-1} + \text{Ei}(e) + e - \text{Ei}(1)
\]

### Step 4: Combine with the First Integral
Now, the original integral is:

\[
\int_0^1 e^{e^x} \, dx - \left( - e^{e-1} + \text{Ei}(e) + e - \text{Ei}(1) \right)
\]

The first integral \( \int_0^1 e^{e^x} \, dx \) can be expressed in terms of the exponential integral as well. Let \( u = e^x \), so \( du = e^x \, dx \), and \( dx = \frac{du}{u} \). The limits are \( x = 0 \to u = 1 \), \( x = 1 \to u = e \):

\[
\int_0^1 e^{e^x} \, dx = \int_1^e \frac{e^{u}}{u} \, du = \text{Ei}(e) - \text{Ei}(1)
\]

### Step 5: Final Simplification
Substitute back:

\[
\left( \text{Ei}(e) - \text{Ei}(1) \right) - \left( - e^{e-1} + \text{Ei}(e) + e - \text{Ei}(1) \right)
\]

Simplify:

\[
\text{Ei}(e) - \text{Ei}(1) + e^{e-1} - \text{Ei}(e) - e + \text{Ei}(1) = e^{e-1} - e
\]

Thus, the exact answer is:

\[
e^{e-1} - e
\]

### Step 6: Numerical Approximation
Compute \( e^{e-1} - e \):

\[
e^{e-1} \approx e^{1.718281828} \approx 5.574941524
\]
\[
e \approx 2.718281828
\]
\[
e^{e-1} - e \approx 5.574941524 - 2.718281828 \approx 2.856659696
\]

Rounded to 10 decimal places:

\[
2.8566596962
\]

### Final Answer
```json
{"answer": "e^{e-1} - e", "numerical_answer": "2.8566596962"}
```