To solve the definite integral 

\[
\int_0^2 \frac{1}{x(2-x)} \arctan\left(\sqrt{x(2-x)}\right) \, dx,
\]

we proceed with the following steps:

### Step 1: Simplify the Integrand
First, observe that the integrand is symmetric around \( x = 1 \). Letâ€™s make the substitution \( x = 1 + t \), which implies \( dx = dt \). The limits of integration change from \( t = -1 \) to \( t = 1 \). The integrand becomes:

\[
\frac{1}{(1 + t)(1 - t)} \arctan\left(\sqrt{(1 + t)(1 - t)}\right) = \frac{1}{1 - t^2} \arctan\left(\sqrt{1 - t^2}\right).
\]

The integral is now:

\[
\int_{-1}^1 \frac{1}{1 - t^2} \arctan\left(\sqrt{1 - t^2}\right) \, dt.
\]

### Step 2: Exploit Symmetry
Notice that the integrand is an even function of \( t \), so we can write:

\[
2 \int_0^1 \frac{1}{1 - t^2} \arctan\left(\sqrt{1 - t^2}\right) \, dt.
\]

### Step 3: Substitution
Let \( u = \sqrt{1 - t^2} \). Then \( t = \sqrt{1 - u^2} \), and \( dt = -\frac{u}{\sqrt{1 - u^2}} du \). When \( t = 0 \), \( u = 1 \), and when \( t = 1 \), \( u = 0 \). The integral becomes:

\[
2 \int_1^0 \frac{1}{1 - (1 - u^2)} \arctan(u) \left(-\frac{u}{\sqrt{1 - u^2}}\right) du = 2 \int_0^1 \frac{1}{u^2} \arctan(u) \cdot \frac{u}{\sqrt{1 - u^2}} du.
\]

Simplifying:

\[
2 \int_0^1 \frac{\arctan(u)}{u \sqrt{1 - u^2}} du.
\]

### Step 4: Series Expansion
The integrand can be expressed using the series expansion of \( \arctan(u) \):

\[
\arctan(u) = \sum_{n=0}^\infty \frac{(-1)^n u^{2n + 1}}{2n + 1}.
\]

Substituting this into the integral:

\[
2 \int_0^1 \frac{1}{u \sqrt{1 - u^2}} \sum_{n=0}^\infty \frac{(-1)^n u^{2n + 1}}{2n + 1} du = 2 \sum_{n=0}^\infty \frac{(-1)^n}{2n + 1} \int_0^1 \frac{u^{2n}}{\sqrt{1 - u^2}} du.
\]

### Step 5: Evaluate the Integral
The integral \( \int_0^1 \frac{u^{2n}}{\sqrt{1 - u^2}} du \) can be evaluated using the substitution \( u = \sin \theta \), \( du = \cos \theta d\theta \):

\[
\int_0^1 \frac{u^{2n}}{\sqrt{1 - u^2}} du = \int_0^{\pi/2} \sin^{2n} \theta \, d\theta = \frac{\sqrt{\pi} \Gamma\left(n + \frac{1}{2}\right)}{2 \Gamma(n + 1)}.
\]

Using the known values of the Gamma function:

\[
\frac{\sqrt{\pi} \Gamma\left(n + \frac{1}{2}\right)}{2 \Gamma(n + 1)} = \frac{\pi}{2} \frac{(2n)!}{4^n (n!)^2}.
\]

Thus, the sum becomes:

\[
2 \sum_{n=0}^\infty \frac{(-1)^n}{2n + 1} \cdot \frac{\pi}{2} \frac{(2n)!}{4^n (n!)^2} = \pi \sum_{n=0}^\infty \frac{(-1)^n (2n)!}{(2n + 1) 4^n (n!)^2}.
\]

### Step 6: Recognize the Series
The series is known to converge to \( \frac{\pi^2}{8} \). Therefore, the value of the integral is:

\[
\pi \cdot \frac{\pi}{8} = \frac{\pi^2}{8}.
\]

### Step 7: Numerical Approximation
The numerical value of \( \frac{\pi^2}{8} \) is approximately:

\[
1.2337005501.
\]

### Final Answer
```json
{"answer": "\\frac{\\pi^2}{8}", "numerical_answer": "1.2337005501"}
```