<think>
Okay, let's tackle this integral ∫ from -4 to 4 of e^|x| times the fractional part of x, dx. Hmm, the fractional part function {x} is x minus the floor of x, right? But since we're dealing with the integral from -4 to 4, I need to consider how the fractional part behaves for negative and positive x. Wait, the fractional part of a negative number isn't the same as for positive. For example, {2.3} is 0.3, but {-2.3} is 0.7 because -2.3 = -3 + 0.7. So, {x} = x - floor(x), which for negative x, floor(x) is the next lower integer. So, for x in [-4, -3), {x} = x - (-4) = x +4. Wait, let me check. If x is -3.5, floor(x) is -4, so {x} = x - (-4) = x +4. So in the interval [-4, -3), {x} = x +4. Similarly, in [-3, -2), {x} = x +3, and so on. For positive x, like in [0,1), {x} = x, [1,2) it's x-1, etc. So the integral from -4 to 4 can be broken into intervals where {x} has different expressions. Let's list all the intervals where the fractional part changes its formula.

From -4 to -3: {x} = x +4
From -3 to -2: {x} = x +3
From -2 to -1: {x} = x +2
From -1 to 0: {x} = x +1
From 0 to 1: {x} = x
From 1 to 2: {x} = x -1
From 2 to 3: {x} = x -2
From 3 to 4: {x} = x -3

Wait, but each interval is of length 1, right? So the integral can be split into 8 intervals: from -4 to -3, -3 to -2, ..., 3 to 4. Each of these intervals will have a different expression for {x}, and since e^|x| is also behave differently depending on whether x is negative or positive. Let's note that |x| is equal to -x when x is negative, and x when x is positive. So for x in [-4,0), |x| = -x, and for x in [0,4], |x| = x. Therefore, e^|x| is e^{-x} for x negative and e^x for x positive.

So combining these two aspects, the integral can be split into 8 parts, each part being over an interval of length 1, and in each interval, we can express {x} and e^|x| accordingly. Let's list each interval and the corresponding expressions:

1. [-4, -3): {x} = x +4, |x| = -x → e^{-x}
2. [-3, -2): {x} = x +3, |x| = -x → e^{-x}
3. [-2, -1): {x} = x +2, |x| = -x → e^{-x}
4. [-1, 0): {x} = x +1, |x| = -x → e^{-x}
5. [0, 1): {x} = x, |x| = x → e^{x}
6. [1, 2): {x} = x -1, |x| = x → e^{x}
7. [2, 3): {x} = x -2, |x| = x → e^{x}
8. [3, 4): {x} = x -3, |x| = x → e^{x}

Wait, but the integral is from -4 to 4, so the upper limit is 4. The last interval is [3,4], which is correct. Now, each of these intervals can be integrated separately, and then summed up. Let's compute each integral one by one.

First, let's handle the negative intervals (1 to 4):

Integral 1: ∫ from -4 to -3 of e^{-x}*(x +4) dx
Integral 2: ∫ from -3 to -2 of e^{-x}*(x +3) dx
Integral 3: ∫ from -2 to -1 of e^{-x}*(x +2) dx
Integral 4: ∫ from -1 to 0 of e^{-x}*(x +1) dx

Then the positive intervals (5 to 8):

Integral 5: ∫ from 0 to 1 of e^{x}*x dx
Integral 6: ∫ from 1 to 2 of e^{x}*(x -1) dx
Integral 7: ∫ from 2 to 3 of e^{x}*(x -2) dx
Integral 8: ∫ from 3 to 4 of e^{x}*(x -3) dx

Now, let's compute each integral. Let's start with the negative intervals.

For Integral 1: ∫_{-4}^{-3} e^{-x}(x +4) dx

Let me make a substitution to simplify. Let u = -x, so when x = -4, u = 4; x = -3, u =3. Then dx = -du. The integral becomes:

∫_{4}^{3} e^{u}*(-u +4)(-du) = ∫_{3}^{4} e^{u}(-u +4) du = ∫_{3}^{4} e^{u}(4 - u) du

Similarly, maybe integrating by parts. Let’s consider integrating (4 - u)e^u. Let’s set:

Let’s let v = 4 - u, dv = -du
dw = e^u du, w = e^u

Integration by parts: v*w - ∫w*dv = (4 - u)e^u - ∫e^u*(-du) = (4 - u)e^u + e^u + C = (5 - u)e^u + C

So the integral from 3 to 4 is [(5 - u)e^u] from 3 to 4 = (5 -4)e^4 - (5 -3)e^3 = e^4 - 2e^3

Similarly, Integral 1 is e^4 - 2e^3

Wait, let me check that again. Wait, when we do the integration by parts:

∫(4 - u)e^u du = (4 - u)e^u + ∫e^u du = (4 - u)e^u + e^u + C = (5 - u)e^u + C

Yes, correct. So evaluated from 3 to 4:

At u=4: (5 -4)e^4 = e^4

At u=3: (5 -3)e^3 = 2e^3

So the integral is e^4 - 2e^3

Similarly, Integral 1 is e^4 - 2e^3

Now Integral 2: ∫_{-3}^{-2} e^{-x}(x +3) dx

Again, substitute u = -x, so when x=-3, u=3; x=-2, u=2. dx = -du. Integral becomes:

∫_{3}^{2} e^{u}(-u +3)(-du) = ∫_{2}^{3} e^{u}(3 - u) du

Again, integrate (3 - u)e^u. Let’s do the same by parts:

v = 3 - u, dv = -du
dw = e^u du, w = e^u

Integral becomes (3 - u)e^u + ∫e^u du = (3 - u)e^u + e^u + C = (4 - u)e^u + C

Evaluated from 2 to 3:

At u=3: (4 -3)e^3 = e^3

At u=2: (4 -2)e^2 = 2e^2

So Integral 2 is e^3 - 2e^2

Similarly, Integral 3: ∫_{-2}^{-1} e^{-x}(x +2) dx

Substitute u = -x, x from -2 to -1 → u from 2 to 1. Integral becomes ∫_{2}^{1} e^{u}(-u +2)(-du) = ∫_{1}^{2} e^{u}(2 - u) du

Integrate (2 - u)e^u:

v = 2 - u, dv = -du
dw = e^u du, w = e^u

Integral: (2 - u)e^u + ∫e^u du = (2 - u)e^u + e^u + C = (3 - u)e^u + C

Evaluated from 1 to 2:

At u=2: (3 -2)e^2 = e^2

At u=1: (3 -1)e^1 = 2e

So Integral 3 is e^2 - 2e

Integral 4: ∫_{-1}^{0 e^{-x}(x +1) dx

Again, substitute u = -x, x from -1 to 0 → u from 1 to 0. Integral becomes ∫_{1}^{0} e^{u}(-u +1)(-du) = ∫_{0}^{1} e^{u}(1 - u) du

Integrate (1 - u)e^u:

v = 1 - u, dv = -du
dw = e^u du, w = e^u

Integral: (1 - u)e^u + ∫e^u du = (1 - u)e^u + e^u + C = (2 - u)e^u + C

Evaluated from 0 to 1:

At u=1: (2 -1)e^1 = e

At u=0: (2 -0)e^0 = 2*1 = 2

So Integral 4 is e - 2

Now, summing up the negative side integrals:

Integral1 + Integral2 + Integral3 + Integral4 = (e^4 - 2e^3) + (e^3 - 2e^2) + (e^2 - 2e) + (e - 2)

Let's compute this:

e^4 -2e^3 + e^3 -2e^2 + e^2 -2e + e -2

Combine like terms:

e^4 - e^3 - e^2 - e -2

Now, moving to the positive intervals (5 to 8):

Integral5: ∫0^1 e^x * x dx

Integrate by parts. Let u = x, dv = e^x dx. Then du = dx, v = e^x.

Integral = x e^x | from 0 to1 - ∫0^1 e^x dx = (1*e^1 - 0*e^0) - (e^1 - e^0) = e - (e -1) = e - e +1 =1

Integral5 is 1

Integral6: ∫1^2 e^x (x -1) dx

Let’s substitute t = x -1, so when x=1, t=0; x=2, t=1. Then dx=dt. The integral becomes ∫0^1 e^{t+1} * t dt = e ∫0^1 t e^t dt

Again, integrate by parts. Let u = t, dv = e^t dt. Then du = dt, v = e^t.

Integral = e [ t e^t | from 0 to1 - ∫0^1 e^t dt ] = e [ (1*e^1 -0) - (e^1 - e^0) ] = e [ e - (e -1) ] = e [1] = e

So Integral6 is e

Integral7: ∫2^3 e^x (x -2) dx

Similarly, substitute t = x -2, x=2 → t=0, x=3 → t=1. Integral becomes ∫0^1 e^{t+2} * t dt = e^2 ∫0^1 t e^t dt

Same as before, integral is e^2 [ t e^t - e^t ] from 0 to1 = e^2 [ (e - e) - (0 -1) ] = e^2 [ 0 - (-1) ] = e^2 *1) = e^2

Integral7 is e^2

Integral8: ∫3^4 e^x (x -3) dx

Substitute t = x -3, x=3 → t=0, x=4 → t=1. Integral becomes ∫0^1 e^{t+3} * t dt = e^3 ∫0^1 t e^t dt

Again, same as before, integral is e^3 [ t e^t - e^t ] from 0 to1 = e^3 [ (e - e) - (0 -1) ] = e^3 [ 0 +1 ] = e^3

Integral8 is e^3

Now, summing up the positive side:

Integral5 + Integral6 + Integral7 + Integral8 =1 + e + e^2 + e^3

Now, total integral is sum of negative side and positive side:

Negative side: e^4 - e^3 - e^2 - e -2

Positive side:1 + e + e^2 + e^3

Adding them together:

(e^4 - e^3 - e^2 - e -2) + (1 + e + e^2 + e^3) = e^4 - e^3 - e^2 - e -2 +1 + e + e^2 + e^3

Simplify term by term:

e^4

- e^3 + e^3 = 0

- e^2 + e^2 =0

- e + e =0

-2 +1 = -1

So total integral is e^4 -1

Wait, that's interesting. All the middle terms cancel out, leaving e^4 -1 -2 +1? Wait, wait, let me check again.

Wait, the negative side is e^4 - e^3 - e^2 - e -2

Positive side is 1 + e + e^2 + e^3

Adding:

e^4 + (-e^3 + e^3) + (-e^2 + e^2) + (-e + e) + (-2 +1) = e^4 +0 +0 +0 -1 = e^4 -1

Yes, exactly. So the total integral is e^4 -1.

But wait, that seems too simple. Let me verify each step again.

Negative side integrals sum to e^4 - e^3 - e^2 - e -2

Positive side integrals sum to 1 + e + e^2 + e^3

Adding them:

e^4 - e^3 - e^2 - e -2 +1 + e + e^2 + e^3

Combine like terms:

e^4 + (-e^3 + e^3) + (-e^2 + e^2) + (-e + e) + (-2 +1) = e^4 +0 +0 +0 -1 = e^4 -1

Yes, that's correct. So the exact value is e^4 -1.

Now, the numerical approximation. Let's compute e^4 first. e is approximately 2.718281828459045.

e^4 = (e^2)^2 ≈ (7.3890560989306495)^2 ≈ 54.598150033144236

So e^4 -1 ≈ 54.598150033144236 -1 = 53.598150033144236

Rounded to 10 decimal places: 53.5981500331

Wait, let me check with more precise calculation.

But maybe using a calculator:

e^4 ≈ 54.598150033144236

So 54.598150033144236 -1 =53.598150033144236

Rounded to 10 decimal places: 53.5981500331

Yes, that's correct.

So the exact answer is e^4 -1, and the numerical approximation is approximately 53.5981500331.

But wait, let me check if I made a mistake in the integration steps. Because the result seems surprisingly simple. Let me verify with a different approach.

Alternative approach: Since the function e^{|x|}*{x} is periodic with period 1? Wait, no, {x} has period 1, but e^{|x|} is not periodic. However, the integral is from -4 to 4, which is symmetric around 0, but the function isn't even or odd. Wait, but the integral over [-4,4] can be split into [-4,0] and [0,4]. Let's see:

But in the previous calculation, we split into 8 intervals and found that the sum simplifies to e^4 -1. Let me check if that's correct.

Alternatively, perhaps there's a pattern. For the negative intervals, each integral from -n to -(n-1) (n=1 to4) contributes e^{n} - 2e^{n-1}, and for positive intervals, each integral from n-1 to n contributes e^{n-1}. Wait, maybe not. But in any case, the previous step-by-step integration seems correct, and the result is e^4 -1.

Alternatively, let's check with a numerical approximation. Let's compute the integral numerically using approximate methods for each interval and see if it sums to approximately 53.59815.

But given that e^4 is about 54.59815, subtracting 1 gives 53.59815, which seems plausible.

Therefore, the exact answer is e^4 -1, and the numerical approximation is approximately 53.5981500331.
</think>

{"answer": "e^{4} - 1", "numerical_answer": "53.5981500331"}