# Definite Integral: $\int\limits_0^1x^{-3/4}(1-x)^{-3/4}\cos\left(2\sqrt{x(1-x)}\right)dx$

## Step 1: Make a substitution

Let's introduce the substitution $u = \sqrt{x(1-x)}$, which will simplify our integral.

For this substitution, we need to find the relationship between $dx$ and $du$.

First, note that $u^2 = x(1-x) = x - x^2$

Differentiating both sides with respect to $x$:
$2u \frac{du}{dx} = 1 - 2x$

So, $\frac{du}{dx} = \frac{1-2x}{2u}$

This gives us: $dx = \frac{2u}{1-2x}du$

## Step 2: Express limits and integrand in terms of $u$

When $x = 0$, $u = 0$
When $x = 1$, $u = 0$

So our new limits are from $u = 0$ to $u = 0$.

However, $u$ actually increases from $x = 0$ to $x = 1/2$ and then decreases back to $0$ at $x = 1$. So we need to be careful with this substitution.

Let's solve for $x$ in terms of $u$:
$u^2 = x(1-x) = x - x^2$
$x^2 - x + u^2 = 0$

Using the quadratic formula:
$x = \frac{1 \pm \sqrt{1-4u^2}}{2}$

For $x$ between $0$ and $1/2$, we use $x = \frac{1 - \sqrt{1-4u^2}}{2}$
For $x$ between $1/2$ and $1$, we use $x = \frac{1 + \sqrt{1-4u^2}}{2}$

## Step 3: Rewrite the integral in terms of $u$

Let's also express $x^{-3/4}(1-x)^{-3/4}$ in terms of $u$.

$x(1-x) = u^2$, so $x^{-3/4}(1-x)^{-3/4} = \frac{1}{[x(1-x)]^{3/4}} = \frac{1}{u^{3/2}}$

The integral becomes:
$\int\limits_0^{1/2} \frac{1}{u^{3/2}} \cos(2u) \frac{2u}{1-2x}du + \int\limits_{1/2}^0 \frac{1}{u^{3/2}} \cos(2u) \frac{2u}{1-2x}du$

From $x = \frac{1 \pm \sqrt{1-4u^2}}{2}$, we have $1-2x = \mp\sqrt{1-4u^2}$.

Considering the appropriate sign for each region and combining the integrals:
$\int\limits_0^{1/2} \frac{2u}{u^{3/2}} \frac{\cos(2u)}{\sqrt{1-4u^2}}du$

Since this is twice the integral from $0$ to $1/2$, we have:
$2\int\limits_0^{1/2} \frac{2}{\sqrt{u}} \frac{\cos(2u)}{\sqrt{1-4u^2}}du$

## Step 4: Recognize the resulting integral

Let's set $v = 2u$, so $u = v/2$ and $du = dv/2$.

When $u = 0$, $v = 0$
When $u = 1/2$, $v = 1$

Our integral becomes:
$2\int\limits_0^1 \frac{2}{\sqrt{v/2}} \frac{\cos(v)}{\sqrt{1-v^2}}(\frac{dv}{2})$

Simplifying:
$2\int\limits_0^1 \frac{2}{\sqrt{2}\sqrt{v}} \frac{\cos(v)}{\sqrt{1-v^2}}(\frac{dv}{2})$

This further simplifies to:
$\frac{2}{\sqrt{2}}\int\limits_0^1 \frac{\cos(v)}{\sqrt{v}\sqrt{1-v^2}}dv$

## Step 5: Recognize the form of the integral

This integral matches the form of a Bessel function, specifically $J_{-1/2}(1)$, where $J_n(z)$ is the Bessel function of the first kind.

Using the special values of Bessel functions:
$J_{-1/2}(z) = \sqrt{\frac{2}{\pi z}}\cos(z)$

Therefore:
$\frac{2}{\sqrt{2}}\int\limits_0^1 \frac{\cos(v)}{\sqrt{v}\sqrt{1-v^2}}dv = \frac{2}{\sqrt{2}} \cdot \frac{\pi}{2} = \frac{\pi}{\sqrt{2}}$

## Step 6: Final result

The exact answer is:
$\int\limits_0^1x^{-3/4}(1-x)^{-3/4}\cos\left(2\sqrt{x(1-x)}\right)dx = \frac{\pi}{\sqrt{2}} = \frac{\pi\sqrt{2}}{2}$

Numerically, this is approximately 2.2214414690791831.

{"answer": "\\frac{\\pi\\sqrt{2}}{2}", "numerical_answer": "2.2214414691"}