
To solve the definite integral \(\int_{0}^{1}\arcsin\left(\frac{1}{2}x\right)\arccos(x)\,dx\), we use integration by parts and properties of elliptic integrals. Here are the key steps:

### Step 1: Integration by Parts
Let \(u = \arcsin\left(\frac{1}{2}x\right)\) and \(dv = \arccos(x)\,dx\). Then:
- \(du = \frac{1}{\sqrt{4 - x^2}}\,dx\) (derivative of \(\arcsin\left(\frac{1}{2}x\right)\)),
- \(v = x\arccos(x) - \sqrt{1 - x^2}\) (integral of \(\arccos(x)\)).

By integration by parts:
\[
\int u\,dv = uv\bigg|_{0}^{1} - \int v\,du
\]

### Step 2: Evaluate Boundary Term \(uv\big|_{0}^{1}\)
- At \(x=1\): \(u(1) = \arcsin\left(\frac{1}{2}\right) = \frac{\pi}{6}\), \(v(1) = 1 \cdot 0 - 0 = 0\), so \(uv = 0\).
- At \(x=0\): \(u(0) = \arcsin(0) = 0\), \(v(0) = 0 \cdot \frac{\pi}{2} - 1 = -1\), so \(uv = 0\).

Thus, \(uv\big|_{0}^{1} = 0 - 0 = 0\).

### Step 3: Simplify the Remaining Integral
The integral reduces to:
\[
- \int_{0}^{1} \left(x\arccos(x) - \sqrt{1 - x^2}\right) \cdot \frac{1}{\sqrt{4 - x^2}}\,dx
\]
Split into two integrals:
\[
- \int_{0}^{1} \frac{x\arccos(x)}{\sqrt{4 - x^2}}\,dx + \int_{0}^{1} \frac{\sqrt{1 - x^2}}{\sqrt{4 - x^2}}\,dx
\]

### Step 4: Evaluate the First Integral (\(I_1\))
Let \(u = \arccos(x)\) and \(dv = \frac{x}{\sqrt{4 - x^2}}\,dx\). Then:
- \(du = -\frac{1}{\sqrt{1 - x^2}}\,dx\),
- \(v = -\sqrt{4 - x^2}\) (integral of \(dv\)).

By integration by parts:
\[
I_1 = \pi - \int_{0}^{1} \frac{\sqrt{4 - x^2}}{\sqrt{1 - x^2}}\,dx
\]

### Step 5: Evaluate the Second Integral (\(I_2\))
Using substitution \(x = \sin\theta\), \(dx = \cos\theta\,d\theta\), the integral transforms to:
\[
I_2 = \int_{0}^{\pi/2} \frac{\cos^2\theta}{\sqrt{4 - \sin^2\theta}}\,d\theta
\]
Using \(\cos^2\theta = (4 - \sin^2\theta) - 3\), we split \(I_2\) into:
\[
I_2 = \int_{0}^{\pi/2} \sqrt{4 - \sin^2\theta}\,d\theta - 3\int_{0}^{\pi/2} \frac{1}{\sqrt{4 - \sin^2\theta}}\,d\theta
\]

### Step 6: Express in Terms of Elliptic Integrals
The integrals simplify using complete elliptic integrals of the first (\(K\)) and second (\(E\)) kinds with modulus \(k = \frac{1}{2}\):
- \(\int_{0}^{\pi/2} \sqrt{4 - \sin^2\theta}\,d\theta = 2E\left(\frac{1}{2}\right)\),
- \(\int_{0}^{\pi/2} \frac{1}{\sqrt{4 - \sin^2\theta}}\,d\theta = \frac{1}{2}K\left(\frac{1}{2}\right)\).

### Step 7: Combine Results
The original integral becomes:
\[
- \pi + 4E\left(\frac{1}{2}\right) - \frac{3}{2}K\left(\frac{1}{2}\right)
\]

### Numerical Approximation
Using \(K\left(\frac{1}{2}\right) \approx 1.6857503548\) and \(E\left(\frac{1}{2}\right) \approx 1.4674622510\):
\[
- \pi + 4(1.4674622510) - \frac{3}{2}(1.6857503548) \approx 0.1996308181
\]

{"answer": "\(-\pi + 4E\left(\frac{1}{2}\right) - \frac{3}{2}K\left(\frac{1}{2}\right)\)", "numerical_answer": "0.1996308181"}