We start with the integral

  I = ∫₀² x^(–1/2) (2 – x)^(–1/2) [1 – 0.5 · x(2 – x)] dx.

Step 1. Substitute x = 2 sin²θ.
  Then, when x = 0, sin²θ = 0 ⟹ θ = 0, and when x = 2, sin²θ = 1 ⟹ θ = π/2.
  The derivative is dx = 4 sinθ cosθ dθ.
  Also, note that:
   √x = √(2 sin²θ) = √2 sinθ  and  √(2 – x) = √(2 – 2 sin²θ) = √(2 cos²θ) = √2 cosθ.

Step 2. Rewrite the integrand in terms of θ.
  The factors x^(–1/2) and (2 – x)^(–1/2) become:
   x^(–1/2)(2 – x)^(–1/2) = 1/(√x √(2 – x)) = 1/( (√2 sinθ)(√2 cosθ) ) = 1/(2 sinθ cosθ)

The integrand dx now becomes:
  [1 – 0.5·x(2 – x)] dx  = [1 – 0.5·(2 sin²θ)(2 cos²θ)] (4 sinθ cosθ dθ)
    = [1 – 2 sin²θ cos²θ] (4 sinθ cosθ dθ)

Multiplying by x^(–1/2)(2 – x)^(–1/2):
  1/(2 sinθ cosθ) * [1 – 2 sin²θ cos²θ] (4 sinθ cosθ dθ)
    = 2 [1 – 2 sin²θ cos²θ] dθ

Step 3. The new limits are from θ = 0 to θ = π/2 so the integral becomes:
  I = 2 ∫₀^(π/2) [1 – 2 sin²θ cos²θ] dθ
    = 2 [∫₀^(π/2) dθ – 2 ∫₀^(π/2) sin²θ cos²θ dθ]

The first integral is straightforward:
  ∫₀^(π/2) dθ = π/2.

For the second integral, note that:
  sin²θ cos²θ = (1/4) sin²(2θ)
so that:
  ∫₀^(π/2) sin²θ cos²θ dθ = 1/4 ∫₀^(π/2) sin²(2θ) dθ

Recall that:
  ∫ sin² u du = (u/2) – (sin(2u)/4) + C.
For u = 2θ we have:
  ∫₀^(π/2) sin²(2θ)dθ = (π/4)
thus:
  ∫₀^(π/2) sin²θ cos²θ dθ = 1/4 · (π/4) = π/16.

Step 4. Substitute these back into I:
  I = 2 [ (π/2) – 2 · (π/16) ]
    = 2 [ (π/2) – (π/8) ]
    = 2 [ (4π – π)/8 ]
    = 2 [ (3π)/8 ]
    = (3π)/4

Thus the exact answer is 3π/4.

Step 5. Numerically, 3π/4 ≈ 3 × 3.141592653589793 / 4 ≈ 2.3561944902.

{"answer": "$\\frac{3\\pi}{4}$", "numerical_answer": "2.3561944902"}