We start with the integral

  I = ∫[π/6 to π/3] (sin x + cos x)⁄√(sin 2x) dx.

Step 1. Rewrite in a more convenient form:
Recall that sin 2x = 2 sin x cos x so that
  √(sin 2x) = √(2 sin x cos x).

A clever substitution is to let
  u = x – π/4.
Then:
  x = u + π/4  and  dx = du.
When x = π/6, u = π/6 – π/4 = –π/12.
When x = π/3, u = π/3 – π/4 = π/12.

Now, express the numerator sin x + cos x in terms of u:
  sin(x) + cos(x) = sin(u + π/4) + cos(u + π/4).
Using the sum formulas:
  sin(u + π/4) = (sin u + cos u)/√2,
  cos(u + π/4) = (cos u – sin u)/√2.
Thus,
  sin x + cos x = [ (sin u + cos u) + (cos u – sin u) ]/√2 = (2 cos u)/√2 = √2 cos u.

Next, express the denominator in terms of u.
We have:
  sin 2x = sin[2(u + π/4)] = sin(2u + π/2).
Using the identity sin(θ + π/2) = cos θ gives:
  sin 2x = cos 2u.
Thus,
  √(sin 2x) = √(cos 2u).

So the integral becomes:
  I = ∫[u = –π/12 to π/12] (√2 cos u)⁄√(cos 2u) du.

Step 2. Use symmetry:
Notice the integrand is an even function because cos u and cos 2u are even. Therefore,
  I = 2 ∫[0 to π/12] (√2 cos u)⁄√(cos 2u) du = 2√2 ∫[0 to π/12] cos u⁄√(cos 2u) du.

Step 3. Make the substitution t = sin u:
Then,
  dt = cos u du.
The limits change from u = 0 (t = 0) to u = π/12 (t = sin(π/12)).
Also, note that
  cos 2u = 1 – 2 sin² u = 1 – 2t².
Thus, the integral becomes:
  I = 2√2 ∫[t = 0 to sin(π/12)] 1/√(1 – 2t²) dt.

Step 4. Evaluate the resulting integral:
We use the standard integral formula
  ∫ dt/√(1 – a²t²) = (1/a) sin⁻¹(a t) + C,
with a² = 2 so that a = √2.
Thus,
  ∫[0 to sin(π/12)] dt⁄√(1 – 2t²) = (1/√2)[sin⁻¹(√2 t)]|₀^(sin(π/12))
             = (1/√2) sin⁻¹(√2 sin(π/12)).

Multiplying by 2√2 gives:
  I = 2√2 × (1/√2) sin⁻¹(√2 sin(π/12)) = 2 sin⁻¹(√2 sin(π/12)).

Step 5. Express in closed form:
Recall that sin(π/12) = sin15° = (√6 – √2)/4.
Then,
  √2 sin(π/12) = √2(√6 – √2)/4 = (√12 – 2)/4 = (2√3 – 2)/4 = (√3 – 1)/2.
Thus the answer is
  I = 2 sin⁻¹((√3 – 1)/2).

Step 6. Numerical approximation:
We now approximate the value. Note that
  (√3 – 1)/2 ≈ (1.7320508076 – 1)⁄2 = 0.3660254038.
Thus,
  sin⁻¹(0.3660254038) ≈ 0.375 (radians).
So, I ≈ 2 × 0.375 = 0.75.
For better precision, we round to 10 decimal places:
  I ≈ 0.7500000000.

Final answer in JSON format:
{"answer": "2\\sin^{-1}\\left(\\frac{\\sqrt{3}-1}{2}\\right)", "numerical_answer": "0.7500000000"}