Let's calculate the integral:
\[
I = \int_0^1 \frac{x-1}{(x+1)\ln x}\,dx
\]

**Step 1: Analytical Calculation**

Let’s try to decompose the numerator:

\[
x-1 = [(x+1) - 2]
\]
So,
\[
\frac{x-1}{(x+1)\ln x} = \frac{(x+1) - 2}{(x+1)\ln x} = \frac{1}{\ln x} - \frac{2}{(x+1)\ln x}
\]
Thus,
\[
I = \int_0^1 \frac{1}{\ln x} dx - 2\int_0^1 \frac{1}{(x+1)\ln x} dx
\]

Let's evaluate these individually.

---

**A. First Integral:**
\[
J_1 = \int_0^1 \frac{1}{\ln x}\, dx
\]

We recall:
\[
\int_0^1 \frac{dx}{\ln x} = -\gamma
\]
where \(\gamma\) is Euler–Mascheroni constant.

---

**B. Second Integral:**
\[
J_2 = \int_0^1 \frac{1}{(x+1)\ln x} dx
\]
Let’s expand \(\frac{1}{x+1}\) in its power series for \(|x| < 1\):
\[
\frac{1}{x+1} = \sum_{n=0}^\infty (-1)^n x^n
\]
So:
\[
\begin{align*}
J_2 &= \int_0^1 \left[\sum_{n=0}^\infty (-1)^n x^n \cdot \frac{1}{\ln x} \right] dx \\
&= \sum_{n=0}^\infty (-1)^n \int_0^1 \frac{x^n}{\ln x} dx
\end{align*}
\]
Recall:
\[
\int_0^1 x^a \frac{dx}{\ln x} = -\frac{1}{a+1}, \quad (\text{for } a > -1)
\]
So for integer \(n \geq 0\),
\[
\int_0^1 \frac{x^n}{\ln x} dx = -\frac{1}{n+1}
\]
Therefore,
\[
J_2 = \sum_{n=0}^\infty (-1)^n \left(-\frac{1}{n+1}\right)
= -\sum_{n=0}^\infty \frac{(-1)^n}{n+1}
\]
But,
\[
\sum_{n=0}^\infty \frac{(-1)^n}{n+1} = \ln 2
\]
So,
\[
J_2 = -\ln 2
\]

---

Now, our original integral becomes:
\[
I = -\gamma - 2(-\ln 2) = -\gamma + 2\ln 2
\]

---

**Step 2: All Steps Given Above!**

---

**Step 3: Numerical Approximation**

\[
\gamma \approx 0.5772156649, \quad \ln 2 \approx 0.6931471806
\]

\[
I \approx -0.5772156649 + 2 \times 0.6931471806 = -0.5772156649 + 1.3862943612 = 0.8090786963
\]

---

**Step 4: JSON Output**

```json
{"answer": "-\\gamma + 2 \\ln 2", "numerical_answer": "0.8090786963"}
```