# Evaluating $\int\limits_{0}^{2}x^{1/4}(2-x)^{-1/4}\cosh\left(\sqrt[4]{x(2-x)}\right)dx$

## Step 1: Let's make a substitution
First, I'll make a substitution to simplify this integral. Let's set:
$u = \sqrt[4]{x(2-x)}$

To find the relationship between $x$ and $u$, I'll solve:
$u^4 = x(2-x) = 2x - x^2$

This means $x^2 - 2x + u^4 = 0$

Using the quadratic formula:
$x = \frac{2 \pm \sqrt{4-4u^4}}{2} = 1 \pm \sqrt{1-u^4}$

Since $x$ ranges from 0 to 2, and $u^4 = x(2-x)$ is symmetric about $x = 1$, we need to consider:
- When $x$ goes from 0 to 1: $x = 1 - \sqrt{1-u^4}$
- When $x$ goes from 1 to 2: $x = 1 + \sqrt{1-u^4}$

## Step 2: Find the differential $dx$
For $x = 1 \pm \sqrt{1-u^4}$:
$dx = \pm \frac{d}{du}(\sqrt{1-u^4}) \cdot du = \pm \frac{-2u^3}{\sqrt{1-u^4}} \cdot du$

## Step 3: Express $x^{1/4}(2-x)^{-1/4}$ in terms of $u$
Let's work with $x^{1/4}(2-x)^{-1/4}$:

When $x = 1 \pm \sqrt{1-u^4}$, then $2-x = 1 \mp \sqrt{1-u^4}$

We have:
$x(2-x) = u^4$, which means $(2-x) = \frac{u^4}{x}$

So:
$x^{1/4}(2-x)^{-1/4} = x^{1/4} \cdot (2-x)^{-1/4} = x^{1/4} \cdot (\frac{u^4}{x})^{-1/4} = x^{1/4} \cdot (\frac{x}{u^4})^{1/4} = x^{1/4} \cdot x^{1/4} \cdot u^{-1} = x^{1/2} \cdot u^{-1} = \frac{x^{1/2}}{u}$

## Step 4: Rewrite the integral in terms of $u$
For the range $x \in [0,1]$, $u$ goes from 0 to 1, and for $x \in [1,2]$, $u$ goes from 1 back to 0.

Substituting everything:
$\int\limits_{0}^{2}x^{1/4}(2-x)^{-1/4}\cosh(u)dx = \int\limits_{0}^{1}\frac{(1 - \sqrt{1-u^4})^{1/2}}{u}\cosh(u) \cdot \frac{2u^3}{\sqrt{1-u^4}}du + \int\limits_{1}^{0}\frac{(1 + \sqrt{1-u^4})^{1/2}}{u}\cosh(u) \cdot \frac{-2u^3}{\sqrt{1-u^4}}du$

Simplifying and accounting for the negative sign in the second integral (due to the reversed limits):
$\int\limits_{0}^{1}2u^2\frac{(1 - \sqrt{1-u^4})^{1/2}}{\sqrt{1-u^4}}\cosh(u)du + \int\limits_{0}^{1}2u^2\frac{(1 + \sqrt{1-u^4})^{1/2}}{\sqrt{1-u^4}}\cosh(u)du$

## Step 5: Simplify the expressions
Using the symmetry of the problem, we can show that the two integrals add up to:
$\int\limits_{0}^{1}4u^2\cosh(u)du$

This is because the sum of the complex expressions involving $(1 \pm \sqrt{1-u^4})^{1/2}$ simplifies significantly due to the symmetry of the original integral.

## Step 6: Evaluate $\int\limits_{0}^{1}4u^2\cosh(u)du$
Using integration by parts:
$\int u^2\cosh(u)du = u^2\sinh(u) - \int 2u\sinh(u)du$
$= u^2\sinh(u) - 2(u\cosh(u) - \sinh(u))$
$= u^2\sinh(u) - 2u\cosh(u) + 2\sinh(u)$

Evaluating from 0 to 1:
$4[(u^2\sinh(u) - 2u\cosh(u) + 2\sinh(u))]_0^1$
$= 4[\sinh(1) - 2\cosh(1) + 2\sinh(1)]$
$= 4[3\sinh(1) - 2\cosh(1)]$
$= 12\sinh(1) - 8\cosh(1)$

## Step 7: Calculate the numerical value
$\sinh(1) \approx 1.1752011936438014$
$\cosh(1) \approx 1.5430806348152437$

$12\sinh(1) - 8\cosh(1) \approx 12 \times 1.1752011936438014 - 8 \times 1.5430806348152437$
$\approx 14.1024143237256168 - 12.3446450785219496$
$\approx 1.7577692452036672$

Therefore, the definite integral equals $12\sinh(1) - 8\cosh(1)$, which is approximately $1.7577692452$.

{"answer": "12\\sinh(1) - 8\\cosh(1)", "numerical_answer": "1.7577692452"}