
To solve the definite integral \(\int_{0}^{2} x \arctan\left(\sqrt{x(2-x)}\right) \, dx\), we proceed as follows:

### Step 1: Simplify the argument of the arctangent
First, rewrite the expression inside the square root:
\[
x(2-x) = 2x - x^2 = 1 - (x-1)^2
\]
Thus, \(\sqrt{x(2-x)} = \sqrt{1 - (x-1)^2}\).

### Step 2: Substitution to exploit symmetry
Let \(t = x - 1\), so \(x = t + 1\) and \(dx = dt\). The limits change from \(x=0\) to \(t=-1\) and \(x=2\) to \(t=1\). The integral becomes:
\[
\int_{-1}^{1} (t + 1) \arctan\left(\sqrt{1 - t^2}\right) \, dt
\]
Split this into two integrals:
\[
\int_{-1}^{1} t \arctan\left(\sqrt{1 - t^2}\right) \, dt + \int_{-1}^{1} \arctan\left(\sqrt{1 - t^2}\right) \, dt
\]

### Step 3: Evaluate the first integral (odd function)
The first integrand \(t \arctan\left(\sqrt{1 - t^2}\right)\) is an odd function (since \(f(-t) = -f(t)\)) and the interval \([-1, 1]\) is symmetric about 0. Thus, the first integral is 0.

### Step 4: Evaluate the second integral (even function)
The second integrand \(\arctan\left(\sqrt{1 - t^2}\right)\) is even (since \(f(-t) = f(t)\)). Thus:
\[
\int_{-1}^{1} \arctan\left(\sqrt{1 - t^2}\right) \, dt = 2 \int_{0}^{1} \arctan\left(\sqrt{1 - t^2}\right) \, dt
\]

### Step 5: Trigonometric substitution
Let \(t = \sin\theta\) (so \(dt = \cos\theta \, d\theta\) and \(\sqrt{1 - t^2} = \cos\theta\)). When \(t=0\), \(\theta=0\); when \(t=1\), \(\theta=\pi/2\). The integral becomes:
\[
2 \int_{0}^{\pi/2} \arctan(\cos\theta) \cdot \cos\theta \, d\theta
\]

### Step 6: Integration by parts
Let \(u = \arctan(\cos\theta)\) and \(dv = \cos\theta \, d\theta\). Then \(du = \frac{-\sin\theta}{1 + \cos^2\theta} \, d\theta\) and \(v = \sin\theta\). Integration by parts gives:
\[
2 \left[ \sin\theta \arctan(\cos\theta) \bigg|_{0}^{\pi/2} + \int_{0}^{\pi/2} \frac{\sin^2\theta}{1 + \cos^2\theta} \, d\theta \right]
\]
The boundary term is 0 (since \(\sin(\pi/2)\arctan(0) = 0\) and \(\sin(0)\arctan(1) = 0\)). Thus, we focus on:
\[
2 \int_{0}^{\pi/2} \frac{\sin^2\theta}{1 + \cos^2\theta} \, d\theta
\]

### Step 7: Simplify the integrand
Using \(\sin^2\theta = 1 - \cos^2\theta\), rewrite the integrand:
\[
\frac{1 - \cos^2\theta}{1 + \cos^2\theta} = \frac{2}{1 + \cos^2\theta} - 1
\]
Thus, the integral becomes:
\[
2 \int_{0}^{\pi/2} \left( \frac{2}{1 + \cos^2\theta} - 1 \right) d\theta = 2 \left( 2 \int_{0}^{\pi/2} \frac{d\theta}{1 + \cos^2\theta} - \int_{0}^{\pi/2} d\theta \right)
\]

### Step 8: Evaluate the remaining integrals
For \(\int_{0}^{\pi/2} \frac{d\theta}{1 + \cos^2\theta}\), use the substitution \(t = \tan\theta\) (so \(d\theta = \frac{dt}{1 + t^2}\) and \(\cos^2\theta = \frac{1}{1 + t^2}\)). The integral becomes:
\[
\int_{0}^{\infty} \frac{1}{1 + \frac{1}{1 + t^2}} \cdot \frac{dt}{1 + t^2} = \int_{0}^{\infty} \frac{dt}{t^2 + 2} = \frac{\pi}{2\sqrt{2}}
\]
Thus:
\[
2 \left( 2 \cdot \frac{\pi}{2\sqrt{2}} - \frac{\pi}{2} \right) = 2 \left( \frac{\pi}{\sqrt{2}} - \frac{\pi}{2} \right) = \pi(\sqrt{2} - 1)
\]

### Final Result
The exact value of the integral is \(\pi(\sqrt{2} - 1)\). A numerical approximation (rounded to 10 decimal places) is approximately \(1.2990381057\).

{"answer": "\(\pi(\sqrt{2} - 1)\)", "numerical_answer": "1.2990381057"}