<think>
Okay, let's tackle this integral step by step. The integral given is ∫₀¹ x^(-1/4) (1 - x)^(1/4) [1 - √(x(1 - x))]^(-2) dx. Hmm, that looks a bit complicated, but maybe there's a substitution that can simplify it.

First, I notice that the integrand has terms involving x and (1 - x) raised to fractional powers, and there's a term with a square root in the denominator. The presence of x and 1 - x suggests that a substitution using the Beta function or Gamma function might be useful here, since those often involve integrals of x^a(1 - x)^b. But the denominator complicates things. Let me see.

The denominator is [1 - √(x(1 - x))]^2. Maybe if I can find a substitution that simplifies this term. Let's try to let t = √(x(1 - x)). Wait, but then dt/dx would involve (1 - 2x)/(2√(x(1 - x))), which might not directly help. Alternatively, perhaps a trigonometric substitution? Let me think. If I set x = sin²θ, then 1 - x = cos²θ, and √(x(1 - x)) = sinθ cosθ. Then the denominator becomes [1 - sinθ cosθ]^2. Hmm, maybe that's a path. Let's try that substitution.

Let x = sin²θ. Then dx = 2 sinθ cosθ dθ. The limits of integration: when x=0, θ=0; when x=1, θ=π/2. Let's substitute into the integrand:

x^(-1/4) = (sin²θ)^(-1/4) = sin^(-1/2)θ

(1 - x)^(1/4) = (cos²θ)^(1/4) = cos^(1/2)θ

Denominator: [1 - sinθ cosθ]^2

So the integrand becomes sin^(-1/2)θ * cos^(1/2)θ * [1 - sinθ cosθ]^(-2) * 2 sinθ cosθ dθ

Simplify the terms:

sin^(-1/2)θ * cos^(1/2)θ * 2 sinθ cosθ = 2 sin^(1/2)θ * cos^(3/2)θ

So the integral becomes ∫₀^(π/2) [2 sin^(1/2)θ cos^(3/2)θ] / [1 - sinθ cosθ]^2 dθ

Hmm, not sure if that's better. Let's see if we can manipulate the denominator. Let's note that 1 - sinθ cosθ. Maybe express sinθ cosθ as (1/2) sin2θ. Then 1 - (1/2) sin2θ. But I don't know if that helps. Alternatively, perhaps another substitution. Let me think.

Alternatively, maybe use substitution t = x/(1 - x). Let's try that. Let t = x/(1 - x), so x = t/(1 + t), and 1 - x = 1/(1 + t). Then dx = [ (1 + t) - t ]/(1 + t)^2 dt = 1/(1 + t)^2 dt. Let's substitute into the integrand:

x^(-1/4) = [t/(1 + t)]^(-1/4) = t^(-1/4) (1 + t)^(1/4)

(1 - x)^(1/4) = [1/(1 + t)]^(1/4) = (1 + t)^(-1/4)

Denominator: [1 - √(x(1 - x))]^2 = [1 - √(t/(1 + t) * 1/(1 + t))]^2 = [1 - √(t)/(1 + t)]^2

So the integrand becomes t^(-1/4) (1 + t)^(1/4) * (1 + t)^(-1/4) * [1 - √t/(1 + t)]^(-2) * 1/(1 + t)^2 dt

Simplify the terms:

t^(-1/4) * (1 + t)^(1/4 - 1/4 - 2) = t^(-1/4) * (1 + t)^(-2)

So the integrand is t^(-1/4) (1 + t)^(-2) [1 - √t/(1 + t)]^(-2) dt

Hmm, not sure if that's better. Let's check the denominator again:

1 - √t/(1 + t) = [ (1 + t) - √t ] / (1 + t) = [1 + t - √t ] / (1 + t)

So [1 - √t/(1 + t)]^(-2) = [ (1 + t) / (1 + t - √t) ]^2

Therefore, the integrand becomes t^(-1/4) (1 + t)^(-2) * [ (1 + t)^2 / (1 + t - √t)^2 ] dt

Simplify:

t^(-1/4) * (1 + t)^(-2) * (1 + t)^2 / (1 + t - √t)^2 = t^(-1/4) / (1 + t - √t)^2 dt

So the integral is ∫₀^∞ t^(-1/4) / (1 + t - √t)^2 dt. Wait, but the original limits when x goes from 0 to 1, t goes from 0 to ∞. Hmm, this might not be helpful. Maybe another substitution.

Alternatively, let's consider the substitution u = √x. Let u = x^(1/2), so x = u², dx = 2u du. Then the integral becomes:

∫₀¹ (u²)^(-1/4) (1 - u²)^(1/4) [1 - u√(1 - u²)]^(-2) * 2u du

Simplify:

u^(-1/2) (1 - u²)^(1/4) [1 - u√(1 - u²)]^(-2) * 2u du = 2 u^(1/2) (1 - u²)^(1/4) [1 - u√(1 - u²)]^(-2) du

Hmm, not sure. Maybe another approach. Let's look back at the original integral:

∫₀¹ x^{-1/4} (1 - x)^{1/4} [1 - √(x(1 - x))]^{-2} dx

Let me check if this can be related to the Beta function. The Beta function is ∫₀¹ t^{c - 1} (1 - t)^{d - 1} dt = B(c, d) = Γ(c)Γ(d)/Γ(c + d). But here, the denominator complicates things. Alternatively, maybe expand the denominator as a series?

The term [1 - √(x(1 - x))]^{-2} can be expanded using a binomial series if |√(x(1 - x))| < 1. Since x is between 0 and 1, √(x(1 - x)) has a maximum at x=1/2, where it's √(1/4) = 1/2. So the maximum value is 1/2, which is less than 1. Therefore, the series converges.

So, [1 - y]^{-2} = Σ_{n=0}^∞ (n + 1) y^n, where y = √(x(1 - x)). Therefore, the integral becomes:

∫₀¹ x^{-1/4} (1 - x)^{1/4} Σ_{n=0}^∞ (n + 1) [√(x(1 - x))]^n dx

= Σ_{n=0}^∞ (n + 1) ∫₀¹ x^{-1/4} (1 - x)^{1/4} [x(1 - x)]^{n/2} dx

Simplify the integrand:

x^{-1/4 + n/2} (1 - x)^{1/4 + n/2}

So the integral becomes Σ_{n=0}^∞ (n + 1) ∫₀¹ x^{n/2 - 1/4} (1 - x)^{n/2 + 1/4} dx

This integral is the Beta function B(n/2 - 1/4 + 1, n/2 + 1/4 + 1) = B(n/2 + 3/4, n/2 + 5/4)

But Beta function B(a, b) = Γ(a)Γ(b)/Γ(a + b). So each term in the series is (n + 1) * Γ(n/2 + 3/4) Γ(n/2 + 5/4) / Γ(n + 2)

But Γ(n/2 + 3/4) Γ(n/2 + 5/4) can be expressed using the duplication formula or other properties. Let's see.

Alternatively, note that Γ(n/2 + 3/4) Γ(n/2 + 5/4) = Γ(n/2 + 3/4) Γ(n/2 + 5/4) = Γ terms with arguments differing by 1/2. There's a formula for Γ(z)Γ(z + 1/2) = 2^{1 - 2z} √π Γ(2z). Let me check:

Yes, the duplication formula is Γ(z)Γ(z + 1/2) = 2^{1 - 2z} √π Γ(2z). Let's apply this with z = n/2 + 3/4.

Then Γ(n/2 + 3/4) Γ(n/2 + 3/4 + 1/2) = Γ(n/2 + 3/4) Γ(n/2 + 5/4) = 2^{1 - 2(n/2 + 3/4)} √π Γ(2(n/2 + 3/4)) = 2^{1 - n - 3/2} √π Γ(n + 3/2) = 2^{-n - 1/2} √π Γ(n + 3/2)

Therefore, substituting back into the series:

(n + 1) * [2^{-n - 1/2} √π Γ(n + 3/2)] / Γ(n + 2)

But Γ(n + 3/2) = (n + 1/2) Γ(n + 1/2) = (n + 1/2)(n - 1/2)...(1/2)√π. Wait, but maybe express Γ(n + 3/2) in terms of factorial. Γ(n + 3/2) = (2n + 1)!! / 2^{n + 1} } √π. Alternatively, perhaps use the relation between Γ(n + 3/2) and Γ(n + 2).

Note that Γ(n + 2) = (n + 1)! and Γ(n + 3/2) = (n + 1/2)(n - 1/2)...(1/2)√π. Let's see:

Γ(n + 3/2) = (n + 1/2) Γ(n + 1/2)

Similarly, Γ(n + 1/2) = (n - 1/2) Γ(n - 1/2), and so on. But this might not directly help. Let's compute the ratio Γ(n + 3/2)/Γ(n + 2). Let's write Γ(n + 3/2) = Γ(n + 2 - 1/2) = (n + 1 - 1/2) Γ(n + 1 - 1/2) = (n + 1/2) Γ(n + 1/2). Similarly, Γ(n + 2) = (n + 1) Γ(n + 1). So the ratio is:

Γ(n + 3/2)/Γ(n + 2) = (n + 1/2) Γ(n + 1/2) / [(n + 1) Γ(n + 1)] = (n + 1/2)/(n + 1) * Γ(n + 1/2)/Γ(n + 1)

But Γ(n + 1) = n! and Γ(n + 1/2) = (2n)! √π / (4^n n!)) from the double factorial relation. Let me recall that Γ(n + 1/2) = (2n)! / (4^n n!) ) √π. So substituting:

Γ(n + 1/2)/Γ(n + 1) = [ (2n)! / (4^n n!) ) √π ] / n! = (2n)! √π / (4^n (n!)^2 )

Therefore, the ratio Γ(n + 3/2)/Γ(n + 2) = (n + 1/2)/(n + 1) * (2n)! √π / (4^n (n!)^2 )

Putting this back into the series term:

Each term is (n + 1) * [2^{-n - 1/2} √π * Γ(n + 3/2) ] / Γ(n + 2) = (n + 1) * 2^{-n - 1/2} √π * [ (n + 1/2) (2n)! √π / (4^n (n!)^2 ) ] / (n + 1)

Wait, the (n + 1) cancels with the denominator (n + 1) from the ratio. So simplifying:

= 2^{-n - 1/2} √π * (n + 1/2) (2n)! √π / (4^n (n!)^2 )

Combine terms:

= 2^{-n - 1/2} * π * (n + 1/2) (2n)! / (4^n (n!)^2 )

Note that 4^n = 2^{2n}, so 4^n = 2^{2n}. Therefore, 2^{-n -1/2} / 4^n = 2^{-n -1/2 - 2n} = 2^{-3n -1/2}

So:

= π * (n + 1/2) (2n)! / (2^{3n + 1/2} (n!)^2 )

But (2n)! / (n!)^2 is the central binomial coefficient, which is equal to (2n choose n). So:

= π * (n + 1/2) * (2n choose n) / 2^{3n + 1/2}

Therefore, the entire series becomes:

Σ_{n=0}^∞ π * (n + 1/2) * (2n choose n) / 2^{3n + 1/2}

Factor out π / 2^{1/2}:

= π / √2 * Σ_{n=0}^∞ (n + 1/2) (2n choose n) / 8^n

Hmm, so we need to compute the sum Σ_{n=0}^∞ (n + 1/2) (2n choose n) / 8^n

Let me see if this sum can be evaluated in closed form. Recall that generating functions for central binomial coefficients often involve 1/√(1 - 4x) or similar. Let's recall that Σ_{n=0}^∞ (2n choose n) x^n = 1/√(1 - 4x) for |x| < 1/4.

Similarly, Σ_{n=0}^∞ (2n choose n) x^n = 1/√(1 - 4x)

Also, the derivative of this generating function can give us terms involving n. Let's compute:

Let S = Σ_{n=0}^∞ (2n choose n) x^n = 1/√(1 - 4x)

Then, the derivative S’ = Σ_{n=1}^∞ n (2n choose n) x^{n-1} = (d/dx) [1/√(1 - 4x)] = (2)/( (1 - 4x)^{3/2} )

Multiply by x to get Σ_{n=1}^∞ n (2n choose n) x^n = 2x / (1 - 4x)^{3/2}

Similarly, our sum is Σ_{n=0}^∞ (n + 1/2) (2n choose n) /8^n = Σ_{n=0}^∞ n (2n choose n) /8^n + (1/2) Σ_{n=0}^∞ (2n choose n)/8^n

Using x = 1/8 in the generating functions:

First term: Σ_{n=0}^∞ n (2n choose n) (1/8)^n = 2*(1/8) / (1 - 4*(1/8))^{3/2} = (1/4) / (1 - 0.5)^{3/2} = (1/4) / (0.5)^{3/2} = (1/4) / ( (√0.5)^3 ) = (1/4) / ( (√2/2)^3 ) = (1/4) / ( (2√2)/8 ) ) = (1/4) * (8)/(2√2) ) = (2)/(√2) = √2

Second term: (1/2) Σ_{n=0}^∞ (2n choose n) (1/8)^n = (1/2) * 1/√(1 - 4*(1/8)) = (1/2) * 1/√(1 - 0.5) = (1/2) * 1/√0.5 = (1/2) * √2 = √2/2

Therefore, the sum is √2 + √2/2 = (3/2)√2

Therefore, the original series is π / √2 * (3/2)√2 = π * 3/2

So the integral equals (3/2)π. Wait, that's 3π/2.

Wait, let me verify the steps again to make sure.

First, the sum S = Σ_{n=0}^∞ (n + 1/2) (2n choose n)/8^n

We split it into Σ n (2n choose n)/8^n + (1/2) Σ (2n choose n)/8^n

For the first part, using the derivative:

Σ_{n=0}^∞ n (2n choose n) x^n = x * d/dx [ Σ_{n=0}^∞ (2n choose n) x^n ] = x * d/dx [1/√(1 - 4x)} ] = x * [ (2)/(1 - 4x)^{3/2} } ]

At x = 1/8, this becomes (1/8) * [ 2 / (1 - 4*(1/8))^{3/2} } ] = (1/8) * 2 / (1 - 0.5)^{3/2} = (1/4) / (0.5)^{3/2} = (1/4) / ( (√0.5)^3 ) = (1/4) / ( ( (√2)/2 )^3 ) = (1/4) / ( (2√2)/8 ) ) = (1/4) * (8)/(2√2) ) = (1/4)*(4/√2) = 1/√2

Wait, wait, this contradicts my previous calculation. Let me redo this step:

(1/8) * 2 / (1 - 0.5)^{3/2} = (1/4) / (0.5)^{3/2}

0.5 is 1/2, so (1/2)^{3/2} = (1/2) * (1/√2) ) = 1/(2√2)

Therefore, (1/4) / (1/(2√2)) ) = (1/4) * 2√2 = √2/2

Ah, so the first term is √2/2

The second term is (1/2) * Σ (2n choose n)/8^n = (1/2) * 1/√(1 - 4*(1/8)) = (1/2) * 1/√(1 - 0.5) = (1/2) * 1/√0.5 = (1/2) * √2 = √2/2

Therefore, total sum S = √2/2 + √2/2 = √2

Then the integral is π / √2 * √2 = π

Wait, that's different from before. So the integral equals π.

Wait, so where did I go wrong earlier? Let's check:

Original series after substitution was:

Σ_{n=0}^∞ (n + 1) * [2^{-n - 1/2} √π Γ(n + 3/2) ] / Γ(n + 2)

Then we expressed Γ(n + 3/2) Γ(n + 5/4) using duplication formula, but wait, no, earlier steps had a mistake. Wait, no, actually, when we applied the duplication formula, we had z = n/2 + 3/4, but perhaps there was a miscalculation there. Alternatively, maybe the mistake was in the substitution steps.

Wait, let's retrace the steps:

After expanding the denominator as a series, we had:

Integral = Σ_{n=0}^∞ (n + 1) * B(n/2 + 3/4, n/2 + 5/4)

Then using the duplication formula on Γ(n/2 + 3/4) Γ(n/2 + 5/4) = 2^{1 - 2(n/2 + 3/4)} √π Γ(2(n/2 + 3/4)) = 2^{1 - n - 3/2} √π Γ(n + 3/2) = 2^{-n - 1/2} √π Γ(n + 3/2)

Then the term becomes (n + 1) * [2^{-n - 1/2} √π Γ(n + 3/2)] / Γ(n + 2)

Then Γ(n + 3/2)/Γ(n + 2) = Γ(n + 3/2)/Γ(n + 2) = (n + 1/2)Γ(n + 1/2)/Γ(n + 2) = (n + 1/2)Γ(n + 1/2)/[(n + 1)!]

But Γ(n + 1/2) = (2n)! √π / (4^n n! )

So Γ(n + 3/2)/Γ(n + 2) = (n + 1/2) * (2n)! √π / (4^n n! ) / (n + 1)! )

= (n + 1/2) * (2n)! √π / (4^n n! (n + 1)! ) )

But (n + 1)! = (n + 1) n!

So this becomes (n + 1/2) * (2n)! √π / (4^n n!^2 (n + 1) )

= (2n)! / (n!^2) * √π (n + 1/2) / (4^n (n + 1) )

Then the term is (n + 1) * 2^{-n - 1/2} √π * [ (2n)! √π (n + 1/2) / (4^n (n + 1) n!^2 ) ]

The (n + 1) cancels, leaving:

2^{-n - 1/2} * π * (n + 1/2) (2n)! / (4^n n!^2 )

But 4^n = 2^{2n}, so 2^{-n -1/2} / 4^n = 2^{-3n -1/2}

Thus, term is π (n + 1/2) (2n choose n) / 2^{3n + 1/2}

Then the sum is Σ_{n=0}^∞ π (n + 1/2) (2n choose n) / 2^{3n + 1/2} = π / 2^{1/2} Σ_{n=0}^∞ (n + 1/2) (2n choose n) / 8^n

Which is π / √2 * Σ_{n=0}^∞ (n + 1/2) (2n choose n) (1/8)^n

Then, as computed, this sum equals √2, so the integral is π / √2 * √2 = π

Wait, so the integral equals π. But earlier when I thought it was 3π/2, that was a mistake. The correct sum is √2, leading to π.

But let's verify the sum again. Let me compute S = Σ_{n=0}^∞ (n + 1/2) (2n choose n) (1/8)^n

We have S = Σ_{n=0}^∞ n (2n choose n) (1/8)^n + (1/2) Σ_{n=0}^∞ (2n choose n) (1/8)^n

First term: Σ_{n=0}^∞ n (2n choose n) x^n = x d/dx Σ (2n choose n) x^n = x d/dx [1/√(1 - 4x)} ] = x * [ (2)/(1 - 4x)^{3/2} } ]

At x = 1/8, this is (1/8) * 2 / (1 - 4*(1/8))^{3/2} = (1/4) / (1 - 0.5)^{3/2} = (1/4) / (0.5)^{3/2} = (1/4) / ( (√0.5)^3 ) = (1/4) / ( (1/√2)^3 ) = (1/4) / (1/(2√2)) ) = (1/4) * 2√2 = √2/2

Second term: (1/2) * Σ (2n choose n) (1/8)^n = (1/2) * 1/√(1 - 4*(1/8)) = (1/2) * 1/√(1 - 0.5) = (1/2) * 1/√0.5 = (1/2) * √2 = √2/2

So total S = √2/2 + √2/2 = √2

Therefore, the integral is π / √2 * √2 = π

So the exact value of the integral is π.

But wait, that seems surprisingly simple. Let me check with a numerical approximation to verify.

Let's compute the integral numerically. Let's approximate ∫₀¹ x^(-1/4) (1 - x)^(1/4) [1 - √(x(1 - x))]^(-2) dx.

We can use numerical integration methods. Let's approximate this using a tool or simple estimation.

Alternatively, since the exact answer is π, which is approximately 3.1415926536. Let's see if the numerical approximation matches.

But to confirm, let's compute the integral numerically. However, since I can't compute it here, but if the analytical result is π, then the numerical approximation should be around 3.1415926536.

But let's check with x=0.5. The integrand at x=0.5 is (0.5)^(-1/4) * (0.5)^(1/4) * [1 - √(0.5*0.5)]^(-2) = (0.5)^(-1/4 + 1/4) * [1 - 0.5]^(-2) = 1 * (0.5)^(-2) = 4. So the integrand at x=0.5 is 4. The function likely has a peak there. But integrating from 0 to 1, the integral being π seems plausible.

Alternatively, if I use substitution t = √(x(1 - x)), but I think the series expansion approach leading to π is correct.

Therefore, the exact answer is π, and the numerical approximation is approximately 3.1415926536.
</think>

{"answer": "\\pi", "numerical_answer": "3.1415926536"}