Let's proceed step by step.

Given:
\[
I = \int_{0}^{1} x^{-1/2}(1-x)^{-1/2} T_{4}\left(\sqrt{x(1-x)}\right) dx
\]
where \(T_{4}(x)\) is the 4th Chebyshev polynomial of the first kind:
\[
T_4(x) = 8x^4 - 8x^2 + 1
\]
so
\[
T_4(\sqrt{x(1-x)}) = 8\left(\sqrt{x(1-x)}\right)^4 - 8\left(\sqrt{x(1-x)}\right)^2 + 1
= 8[x(1-x)]^2 - 8[x(1-x)] + 1
\]
Let's compute:
1. \( [x(1-x)]^2 = x^2 (1 - 2x + x^2) = x^2 - 2x^3 + x^4 \)
2. \( x(1-x) = x - x^2 \)

Therefore,
\[
T_4(\sqrt{x(1-x)}) = 8(x^2 - 2x^3 + x^4) - 8(x - x^2) + 1
= 8x^2 - 16x^3 + 8x^4 - 8x + 8x^2 + 1
= 8x^4 - 16x^3 + 16x^2 - 8x + 1
\]

So the integral becomes:
\[
I = \int_0^1 x^{-1/2}(1-x)^{-1/2} [8x^4 - 16x^3 + 16x^2 - 8x + 1] dx
\]
We can split the integral:
\[
I = 8 \int_0^1 x^{-1/2}(1-x)^{-1/2} x^4 dx -16 \int_0^1 x^{-1/2}(1-x)^{-1/2} x^3 dx 
\]
\[
+16 \int_0^1 x^{-1/2}(1-x)^{-1/2} x^2 dx 
-8 \int_0^1 x^{-1/2}(1-x)^{-1/2} x dx 
+ \int_0^1 x^{-1/2}(1-x)^{-1/2} dx
\]

Each term is a Beta integral:
\[
\int_0^1 x^{p-1}(1-x)^{q-1} dx = B(p, q) = \frac{\Gamma(p)\Gamma(q)}{\Gamma(p+q)}
\]

Now, let's rewrite each term:

1. \( x^{-1/2} x^4 = x^{7/2} \), so the power is \(7/2\).
2. \( x^{-1/2} x^3 = x^{5/2} \)
3. \( x^{-1/2} x^2 = x^{3/2} \)
4. \( x^{-1/2} x = x^{1/2} \)
5. \( x^{-1/2} \) (the base case)

So, in all cases, the other term is \( (1-x)^{-1/2} \).

Thus, the Beta integrals become:

1. \( I_1 = 8 \int_0^1 x^{7/2} (1-x)^{-1/2} dx = 8 B(9/2, 1/2) \)
2. \( I_2 = -16 \int_0^1 x^{5/2} (1-x)^{-1/2} dx = -16 B(7/2, 1/2) \)
3. \( I_3 = 16 \int_0^1 x^{3/2} (1-x)^{-1/2} dx = 16 B(5/2, 1/2) \)
4. \( I_4 = -8 \int_0^1 x^{1/2} (1-x)^{-1/2} dx = -8 B(3/2, 1/2) \)
5. \( I_5 = \int_0^1 x^{-1/2}(1-x)^{-1/2} dx = B(1/2, 1/2) \)

Now, recall:
\[
B(p, q) = \frac{\Gamma(p) \Gamma(q)}{\Gamma(p+q)}
\]

Let us compute each Beta function:

- \( B(a, 1/2) = \frac{\Gamma(a) \Gamma(1/2)}{\Gamma(a+1/2)} \), and \( \Gamma(1/2) = \sqrt{\pi} \).

Let us write all five terms:

1. \( 8 B(9/2, 1/2) = 8 \frac{\Gamma(9/2) \sqrt{\pi}}{\Gamma(5)} \)
2. \(-16 B(7/2, 1/2) = -16 \frac{\Gamma(7/2) \sqrt{\pi}}{\Gamma(4)} \)
3. \(16 B(5/2, 1/2) = 16 \frac{\Gamma(5/2) \sqrt{\pi}}{\Gamma(3)} \)
4. \(-8 B(3/2, 1/2) = -8 \frac{\Gamma(3/2) \sqrt{\pi}}{\Gamma(2)} \)
5. \(B(1/2, 1/2) = \frac{\Gamma(1/2)^2}{\Gamma(1)} = \pi\) (since \(\Gamma(1/2) = \sqrt{\pi}\), and \(\Gamma(1) = 1\))

Let us compute all relevant Gamma values:

- \(\Gamma(1) = 1\)
- \(\Gamma(2) = 1!\! = 1\)
- \(\Gamma(3) = 2! = 2\)
- \(\Gamma(4) = 3! = 6\)
- \(\Gamma(5) = 4! = 24\)

The half-integer Gamma function is:
\[
\Gamma\left(n + \frac{1}{2}\right) = \frac{(2n)!}{n! 2^{2n}} \sqrt{\pi}
\]

Or, specifically:
- \(\Gamma(3/2) = \frac{1}{2} \sqrt{\pi}\)
- \(\Gamma(5/2) = \frac{3}{4} \sqrt{\pi}\)
- \(\Gamma(7/2) = \frac{15}{8} \sqrt{\pi}\)
- \(\Gamma(9/2) = \frac{105}{16} \sqrt{\pi}\)

Let's substitute these:

- \(\Gamma(3/2) = \frac{1}{2} \sqrt{\pi}\)
- \(\Gamma(5/2) = \frac{3}{4} \sqrt{\pi}\)
- \(\Gamma(7/2) = \frac{15}{8} \sqrt{\pi}\)
- \(\Gamma(9/2) = \frac{105}{16} \sqrt{\pi}\)

Plugging in:

1. \( 8 \cdot \frac{\Gamma(9/2) \sqrt{\pi}}{\Gamma(5)} = 8 \cdot \frac{(\frac{105}{16}\sqrt{\pi}) \sqrt{\pi}}{24} = 8 \cdot \frac{105}{16} \cdot \frac{\pi}{24} \)
2. \( -16 \cdot \frac{\Gamma(7/2) \sqrt{\pi}}{\Gamma(4)} = -16 \cdot \frac{(\frac{15}{8}\sqrt{\pi}) \sqrt{\pi}}{6} = -16 \cdot \frac{15}{8} \cdot \frac{\pi}{6} \)
3. \( 16 \cdot \frac{\Gamma(5/2) \sqrt{\pi}}{\Gamma(3)} = 16 \cdot \frac{(\frac{3}{4}\sqrt{\pi}) \sqrt{\pi}}{2} = 16 \cdot \frac{3}{4} \cdot \frac{\pi}{2} \)
4. \( -8 \cdot \frac{\Gamma(3/2) \sqrt{\pi}}{\Gamma(2)} = -8 \cdot \frac{(\frac{1}{2}\sqrt{\pi}) \sqrt{\pi}}{1} = -8 \cdot \frac{1}{2} \cdot \pi \)
5. \( \pi \)

Simplifying all:

1. \( 8 \times \frac{105}{16} \times \frac{\pi}{24} = \frac{8 \times 105 \pi}{16 \times 24} = \frac{840\pi}{384} = \frac{35\pi}{16} \)
2. \( -16 \times \frac{15}{8} \times \frac{\pi}{6} = -16 \times 15 \times \frac{\pi}{8 \times 6} = -240 \times \frac{\pi}{48} = -5 \pi \)
3. \( 16 \times \frac{3}{4} \times \frac{\pi}{2} = 16 \times 3 \pi / 8 = 48\pi/8 = 6\pi \)
4. \( -8 \times \frac{1}{2} \times \pi = -4 \pi \)
5. \( \pi \)

Sum them up:

\[
I = \frac{35\pi}{16} - 5\pi + 6\pi - 4\pi + \pi
\]

Let's sum the coefficients:

\[
\frac{35}{16}\pi - 5\pi + 6\pi - 4\pi + \pi = \frac{35}{16}\pi - 5\pi + 6\pi - 4\pi + \pi
\]
\[
= \frac{35}{16}\pi + (-5+6-4+1)\pi = \frac{35}{16}\pi - 2\pi
\]
\[
= \left(\frac{35}{16} - 2\right)\pi = \left(\frac{35-32}{16}\right)\pi = \frac{3}{16}\pi
\]

Thus,
\[
I = \frac{3\pi}{16}
\]

Now, let's compute the numerical value:

\[
\frac{3\pi}{16} \approx \frac{3 \times 3.141592653589793}{16} \approx \frac{9.424777960769}{16} \approx 0.5890486225
\]

## Final Answers

```json
{"answer": "\\frac{3\\pi}{16}", "numerical_answer": "0.5890486225"}
```