We start with the integral

  I = ∫₀² (1/x)·arctan(√(x(2−x))) dx.

Step 1. Make the substitution x = 2 sin²t. Then
  dx = 4 sin t cos t dt,
  and when x = 0, t = 0; when x = 2, sin²t = 1 so t = π/2.
Also, note
  √(x(2−x)) = √(2 sin²t · 2 cos²t) = 2 sin t cos t,
and the factor 1/x becomes 1/(2 sin²t).

Thus the integrand transforms as follows:
  (1/x) dx = (1/(2 sin²t)) · (4 sin t cos t dt) = (2 cos t/sin t) dt = 2 cot t dt,
and
  arctan(√(x(2−x))) = arctan(2 sin t cos t) = arctan(sin 2t).

Therefore the integral becomes

  I = 2∫₀^(π/2) cot t · arctan(sin 2t) dt.

Step 2. Introduce a parameter. Define for any real a the function

  J(a) = ∫₀² (1/x)·arctan(a√(x(2−x))) dx.
Then I = J(1). Differentiate J(a) with respect to a:

  J′(a) = ∫₀² (1/x) · [1/(1 + a² x(2−x))] · √(x(2−x)) dx.

Again, substitute x = 2 sin²t with the relations listed above. Then
  √(x(2−x)) = 2 sin t cos t,
  x = 2 sin²t,
  dx = 4 sin t cos t dt,
and
  x(2−x) = 4 sin²t cos²t = sin²2t  (since sin 2t = 2 sin t cos t).

Thus
  J′(a) = ∫₀^(π/2) [1/(2 sin²t)] · [1/(1 + a²·(4 sin²t cos²t))] · (2 sin t cos t) · (4 sin t cos t dt).
Combine the factors:
  The product (2 sin t cos t)·(4 sin t cos t) = 8 sin²t cos²t.
Dividing by 2 sin²t gives 4 cos²t. Also, note 4 sin²t cos²t = sin²2t. Hence

  J′(a) = 4∫₀^(π/2) [cos²t/(1 + a² sin²2t)] dt.

Now write cos²t = (1+cos 2t)/2 so that

  J′(a) = 2∫₀^(π/2) [1+cos 2t]/(1 + a² sin²2t) dt.

Make the substitution u = 2t (so that du = 2 dt). When t goes from 0 to π/2, u goes from 0 to π. Then

  J′(a) = 2·(1/2)∫₀^π [1+cos u]/(1 + a² sin²u) du = ∫₀^π [1+cos u]/(1 + a² sin²u) du.

We split the integral into two parts:
  J′(a) = ∫₀^π 1/(1 + a² sin²u) du + ∫₀^π cos u/(1 + a² sin²u) du.

The second integral vanishes by symmetry (by the substitution u → π − u, cos u is antisymmetric while sin²u is symmetric). It is known that

  ∫₀^π du/(1 + a² sin²u) = π/√(1+a²).

Thus we find

  J′(a) = π/√(1+a²).

Now integrate with respect to a:

  J(a) = ∫₀^a [π/√(1+s²)] ds = π·asinh(a)   (since asinh(0)=0).

Recalling that I = J(1), we obtain the closed‐form answer

  I = π·asinh(1) = π·ln(1 + √2).

Step 3. We now provide a numerical approximation. Using

  √2 ≈ 1.4142135624  and  ln(1+√2) ≈ ln(2.4142135624) ≈ 0.881373,
we have

  I ≈ π × 0.881373 ≈ 3.1415926536 × 0.881373 ≈ 2.7690356807.

Step 4. Final Answer in JSON format:

{"answer": "\\pi \\ln\\left(1+\\sqrt{2}\\right)", "numerical_answer": "2.7690356807"}