Let's begin solving the definite integral:

\[
I = \int_0^{2\pi}\tan(\cos(x))\, dx
\]

### Step 1: Analyze the function

First, notice that \(\tan(\cos(x))\) is a periodic function with period \(2\pi\) because \(\cos(x)\) is \(2\pi\)-periodic.

#### Symmetry Analysis

Let’s consider the substitution \(u = 2\pi - x\):

- As \(x\) goes from \(0\) to \(2\pi\), \(u\) goes from \(2\pi\) to \(0\).
- \(du = -dx\)
- \(\cos(u) = \cos(2\pi - x) = \cos(x)\) (since cosine is \(2\pi\)-periodic and even).

The limits swap, so:

\[
\int_0^{2\pi}\tan(\cos(x))\,dx = \int_{2\pi}^{0}\tan(\cos(2\pi - u))\,(-du)
\]
\[
= \int_0^{2\pi}\tan(\cos(u))\, du
\]

No new information; the integral is equal to itself with this substitution.

Let’s consider a more fruitful symmetry:

Let’s analyze the function \(f(x) = \tan(\cos(x))\) over \([0, 2\pi]\).

Try \(x \to 2\pi - x\):

- \(\cos(2\pi - x) = \cos(x)\)
- So, \(f(2\pi - x) = f(x)\)

So, \(f(x)\) is symmetric about \(x = \pi\) on \([0, 2\pi]\).

Now, let’s check \(x \rightarrow \pi + x\):

- \(\cos(\pi + x) = -\cos(x)\)
- So, \(f(\pi + x) = \tan(-\cos(x)) = -\tan(\cos(x))\)

Therefore, over \(x \in [0,\pi]\):

\[
f(x) + f(\pi + x) = \tan(\cos(x)) + \tan(-\cos(x)) = \tan(\cos(x)) - \tan(\cos(x)) = 0
\]

### Step 2: Split the integral

So,

\[
I = \int_0^{2\pi} \tan(\cos(x)) dx = \int_0^{\pi} \tan(\cos(x)) dx + \int_{\pi}^{2\pi} \tan(\cos(x)) dx
\]

Make the substitution \(y = x - \pi\) in the second integral (\(x = \pi \to y = 0\), \(x = 2\pi \to y = \pi\)):

- \(\cos(x) = \cos(y+\pi) = -\cos(y)\)
- \(dx = dy\)

So:

\[
\int_{\pi}^{2\pi} \tan(\cos(x)) \, dx = \int_0^{\pi} \tan(\cos(y+\pi))\,dy = \int_0^{\pi} \tan(-\cos(y))\,dy = -\int_0^{\pi}\tan(\cos(y))\,dy
\]

Therefore,

\[
I = \int_0^{\pi}\tan(\cos(x))\,dx - \int_0^{\pi}\tan(\cos(x))\,dx = 0
\]

### Step 3: Numerical Approximation

Numerically, integrating \(\tan(\cos x)\) from \(0\) to \(2\pi\) should yield 0.

### Step 4: Final Answer in JSON

```json
{"answer": "0", "numerical_answer": "0.0000000000"}
```