To solve the definite integral \(\int_{\frac{1}{4}}^{4} \frac{\tan^{-1}(x)}{x} \, dx\), we will follow the steps outlined.

### Step 1: Compute the Integral Analytically

Consider the integral:
\[ I = \int_{\frac{1}{4}}^{4} \frac{\tan^{-1}(x)}{x} \, dx. \]

We can use the substitution \( u = \tan^{-1}(x) \). Then, \( du = \frac{1}{1 + x^2} \, dx \). However, this substitution does not directly simplify the integral. Instead, we can use a different approach involving the properties of the arctangent function and symmetry.

Notice that:
\[ \tan^{-1}(x) + \tan^{-1}\left(\frac{1}{x}\right) = \frac{\pi}{2} \quad \text{for} \quad x > 0. \]

We can split the integral into two parts and use this property:
\[ I = \int_{\frac{1}{4}}^{1} \frac{\tan^{-1}(x)}{x} \, dx + \int_{1}^{4} \frac{\tan^{-1}(x)}{x} \, dx. \]

For the second integral, we can use the substitution \( t = \frac{1}{x} \), which gives \( dt = -\frac{1}{x^2} \, dx \) and changes the limits of integration accordingly:
\[ \int_{1}^{4} \frac{\tan^{-1}(x)}{x} \, dx = \int_{1}^{\frac{1}{4}} \frac{\tan^{-1}\left(\frac{1}{t}\right)}{\frac{1}{t}} \left(-\frac{1}{t^2}\right) \, dt = \int_{\frac{1}{4}}^{1} \frac{\tan^{-1}\left(\frac{1}{t}\right)}{t} \, dt. \]

Using the property \(\tan^{-1}\left(\frac{1}{t}\right) = \frac{\pi}{2} - \tan^{-1}(t)\), we get:
\[ \int_{\frac{1}{4}}^{1} \frac{\tan^{-1}\left(\frac{1}{t}\right)}{t} \, dt = \int_{\frac{1}{4}}^{1} \frac{\frac{\pi}{2} - \tan^{-1}(t)}{t} \, dt. \]

Thus, the original integral becomes:
\[ I = \int_{\frac{1}{4}}^{1} \frac{\tan^{-1}(x)}{x} \, dx + \int_{\frac{1}{4}}^{1} \frac{\frac{\pi}{2} - \tan^{-1}(x)}{x} \, dx. \]

Combining these integrals, we get:
\[ I = \int_{\frac{1}{4}}^{1} \frac{\tan^{-1}(x)}{x} \, dx + \int_{\frac{1}{4}}^{1} \frac{\frac{\pi}{2}}{x} \, dx - \int_{\frac{1}{4}}^{1} \frac{\tan^{-1}(x)}{x} \, dx. \]

The \(\tan^{-1}(x)\) terms cancel out, leaving:
\[ I = \int_{\frac{1}{4}}^{1} \frac{\frac{\pi}{2}}{x} \, dx = \frac{\pi}{2} \int_{\frac{1}{4}}^{1} \frac{1}{x} \, dx. \]

This integral is straightforward:
\[ \int_{\frac{1}{4}}^{1} \frac{1}{x} \, dx = \ln(1) - \ln\left(\frac{1}{4}\right) = 0 - (-\ln(4)) = \ln(4). \]

Thus:
\[ I = \frac{\pi}{2} \ln(4). \]

Since \(\ln(4) = 2 \ln(2)\), we have:
\[ I = \frac{\pi}{2} \cdot 2 \ln(2) = \pi \ln(2). \]

### Step 2: Numerical Approximation

Using the value of \(\pi \approx 3.141592653589793\) and \(\ln(2) \approx 0.6931471805599453\), we get:
\[ \pi \ln(2) \approx 3.141592653589793 \times 0.6931471805599453 \approx 2.177586090303602. \]

### Step 3: Output the Final Answer in JSON Format

```json
{"answer": "\\pi \\ln(2)", "numerical_answer": "2.1775860903"}
```