Let's compute the definite integral:
\[
I = \int_0^1 \sin(\cos^{-1}(x))\,dx
\]

**Step 1: Simplify the Integrand**

Recall the trigonometric identity:
\[
\sin(\cos^{-1}(x)) = \sqrt{1 - x^2}
\]
because, if \(\theta = \cos^{-1}(x)\), then \(\cos\theta = x\), and by the Pythagorean identity:
\[
\sin\theta = \sqrt{1 - \cos^2\theta} = \sqrt{1 - x^2}
\]

Thus,
\[
I = \int_0^1 \sqrt{1 - x^2} \, dx
\]

**Step 2: Compute the Definite Integral \(\int_0^1 \sqrt{1-x^2} dx\)**

This is the area under the top half of a unit circle from \(x=0\) to \(x=1\).

We use the substitution:

Let \(x = \sin\theta\), \(dx = \cos\theta d\theta\), and as \(x\) goes from 0 to 1, \(\theta\) goes from 0 to \(\frac{\pi}{2}\):

- when \(x = 0\), \(\sin\theta = 0 \implies \theta = 0\)
- when \(x = 1\), \(\sin\theta = 1 \implies \theta = \frac{\pi}{2}\)

Now,
\[
\sqrt{1-x^2} = \sqrt{1 - \sin^2\theta} = \cos\theta
\]
and
\[
dx = \cos\theta\, d\theta
\]
So,
\[
I = \int_{\theta=0}^{\pi/2} \cos\theta \cdot \cos\theta\, d\theta = \int_0^{\pi/2} \cos^2\theta\, d\theta
\]

Recall the power-reduction formula:
\[
\cos^2\theta = \frac{1 + \cos(2\theta)}{2}
\]

Therefore,
\[
I = \int_0^{\pi/2} \frac{1 + \cos(2\theta)}{2} d\theta = \frac{1}{2} \int_0^{\pi/2} 1\, d\theta + \frac{1}{2} \int_0^{\pi/2} \cos(2\theta)\, d\theta
\]

Evaluate each part separately:
\begin{align*}
\int_0^{\pi/2} 1\, d\theta &= \frac{\pi}{2} \\
\int_0^{\pi/2} \cos(2\theta) d\theta &= \left[ \frac{\sin(2\theta)}{2}\right]_0^{\pi/2} \\
&= \frac{\sin(\pi)}{2} - \frac{\sin(0)}{2} \\
&= 0
\end{align*}

Therefore,
\[
I = \frac{1}{2} \cdot \frac{\pi}{2} + \frac{1}{2} \cdot 0 = \frac{\pi}{4}
\]

**Step 3: Numerical Approximation**

\[
\frac{\pi}{4} \approx 0.7853981634
\]

**Step 4: JSON Output**

```json
{"answer": "\\frac{\\pi}{4}", "numerical_answer": "0.7853981634"}
```