Let's proceed step by step.

### 1. **Rewrite the Integral**

\[
I = \int_{64}^{729} \frac{x^{1/2}}{x^{1/2} - x^{1/3}} \, dx
\]

Factor \( x^{1/3} \) from the denominator:

\[
x^{1/2} - x^{1/3} = x^{1/3}(x^{1/6} - 1)
\]

So,

\[
\frac{x^{1/2}}{x^{1/2} - x^{1/3}} = \frac{x^{1/2}}{x^{1/3}(x^{1/6} - 1)} = \frac{x^{1/2-1/3}}{x^{1/6} - 1} = \frac{x^{1/6}}{x^{1/6} - 1}
\]

So the integral simplifies to:

\[
I = \int_{64}^{729} \frac{x^{1/6}}{x^{1/6} - 1} dx
\]

Let \( u = x^{1/6} \implies x = u^6 \implies dx = 6u^5 du \).

Change the limits:

- When \( x = 64 \): \( u = 64^{1/6} = 2 \)
- When \( x = 729 \): \( u = 729^{1/6} = 3 \)

Now, substitute into the integral:

\[
I = \int_{u=2}^{u=3} \frac{u}{u-1} 6u^5 du = 6 \int_2^3 \frac{u^6}{u-1} du
\]

### 2. **Integrate \( \frac{u^6}{u-1} \) **

Let us perform polynomial division:

\[
\frac{u^6}{u-1} = u^5 + u^4 + u^3 + u^2 + u + 1 + \frac{1}{u-1}
\]

So,

\[
\int_2^3 \frac{u^6}{u-1} du = \int_2^3 \left(u^5 + u^4 + u^3 + u^2 + u + 1 + \frac{1}{u-1}\right) du
\]

Integrate each term:

- \(\int u^5 du = \frac{u^6}{6}\)
- \(\int u^4 du = \frac{u^5}{5}\)
- \(\int u^3 du = \frac{u^4}{4}\)
- \(\int u^2 du = \frac{u^3}{3}\)
- \(\int u du = \frac{u^2}{2}\)
- \(\int 1 du = u\)
- \(\int \frac{1}{u-1} du = \ln|u-1|\)

Combine:

\[
F(u) = \frac{u^6}{6} + \frac{u^5}{5} + \frac{u^4}{4} + \frac{u^3}{3} + \frac{u^2}{2} + u + \ln|u-1|
\]

Evaluated from \( u = 2 \) to \( u = 3 \):

\[
I = 6 \left[ F(3) - F(2) \right]
\]

### 3. **Calculate \( F(3) \) and \( F(2) \):**

#### For \( u = 3 \):

- \( 3^6 = 729 \)
- \( 3^5 = 243 \)
- \( 3^4 = 81 \)
- \( 3^3 = 27 \)
- \( 3^2 = 9 \)
- \( 3 - 1 = 2 \)

So,

\[
F(3) = \frac{729}{6} + \frac{243}{5} + \frac{81}{4} + \frac{27}{3} + \frac{9}{2} + 3 + \ln 2
\]

#### For \( u = 2 \):

- \( 2^6 = 64 \)
- \( 2^5 = 32 \)
- \( 2^4 = 16 \)
- \( 2^3 = 8 \)
- \( 2^2 = 4 \)
- \( 2 - 1 = 1 \)

So,

\[
F(2) = \frac{64}{6} + \frac{32}{5} + \frac{16}{4} + \frac{8}{3} + \frac{4}{2} + 2 + \ln 1
\]

But \( \ln 1 = 0 \).

### 4. **Compute the Difference Explicitly:**

\[
I = 6 \Bigg[\left(\frac{729}{6} + \frac{243}{5} + \frac{81}{4} + 9 + 4.5 + 3 + \ln 2\right)
- \left(\frac{64}{6} + \frac{32}{5} + 4 + \frac{8}{3} + 2 + 2\right)\Bigg]
\]

Calculate terms:

- \( \frac{729}{6} = 121.5 \), \( \frac{243}{5} = 48.6 \), \( \frac{81}{4} = 20.25 \), \( \frac{27}{3} = 9 \), \( \frac{9}{2} = 4.5 \), \( 3 \), \( \ln 2 \approx 0.6931471806 \)
- \( \frac{64}{6} = 10.\overline{6} \), \( \frac{32}{5} = 6.4 \), \( \frac{16}{4} = 4 \), \( \frac{8}{3} = 2.\overline{6} \), \( \frac{4}{2} = 2 \), 2

Sum:

First bracket:  
\( 121.5 + 48.6 + 20.25 + 9 + 4.5 + 3 + 0.6931471806 = 207.5431471806 \)

Second bracket:  
\( 10.6666666667 + 6.4 + 4 + 2.6666666667 + 2 + 2 = 27.7333333334 \)

Their difference:

\( 207.5431471806 - 27.7333333334 = 179.8098138472 \)

Multiply by 6:

\(
I = 6 \times 179.8098138472 = 1,078.8588830832
\)

**Round to 10 decimal places:**  
\( \boxed{1078.8588830832} \)

### 5. **Express the Exact Answer in LaTeX**

Exact answer:

\[
I = 6\left[
\left(
\frac{729}{6} + \frac{243}{5} + \frac{81}{4} + 9 + 4.5 + 3 + \ln 2
\right)
-
\left(
\frac{64}{6} + \frac{32}{5} + 4 + \frac{8}{3} + 2 + 2
\right)
\right]
\]

Or, simplify constants where possible:

\[
I = 6\left[
\left(
\frac{729}{6} + \frac{243}{5} + \frac{81}{4} + \frac{27}{3} + \frac{9}{2} + 3 + \ln 2
\right)
-
\left(
\frac{64}{6} + \frac{32}{5} + \frac{16}{4} + \frac{8}{3} + \frac{4}{2} + 2
\right)
\right]
\]

---

```json
{"answer": "6\\left[\\left(\\frac{729}{6} + \\frac{243}{5} + \\frac{81}{4} + \\frac{27}{3} + \\frac{9}{2} + 3 + \\ln 2\\right) - \\left(\\frac{64}{6} + \\frac{32}{5} + \\frac{16}{4} + \\frac{8}{3} + \\frac{4}{2} + 2\\right)\\right]", "numerical_answer": "1078.8588830832"}
```