
To solve the definite integral \(\int_0^1 \left( e^{e^x} - e^{e^x - x} \right) dx\), we proceed as follows:

### Step 1: Split the Integral
First, we split the integral into two separate terms:
\[
\int_0^1 e^{e^x} \, dx - \int_0^1 e^{e^x - x} \, dx
\]

### Step 2: Analyze the First Integral
The first integral is \(\int_0^1 e^{e^x} \, dx\). Using the substitution \(u = e^x\), we have \(du = e^x \, dx\) or \(dx = \frac{du}{u}\). When \(x = 0\), \(u = 1\); when \(x = 1\), \(u = e\). Thus:
\[
\int_0^1 e^{e^x} \, dx = \int_1^e \frac{e^u}{u} \, du
\]
This integral is related to the exponential integral function \(\text{Ei}(u)\), where \(\text{Ei}(u) = \int_{-\infty}^u \frac{e^t}{t} \, dt\). Thus:
\[
\int_1^e \frac{e^u}{u} \, du = \text{Ei}(e) - \text{Ei}(1)
\]

### Step 3: Analyze the Second Integral
The second integral is \(\int_0^1 e^{e^x - x} \, dx\). Rewrite the integrand as \(e^{e^x} \cdot e^{-x}\). Using the same substitution \(u = e^x\) (so \(e^{-x} = \frac{1}{u}\) and \(dx = \frac{du}{u}\)), the integral becomes:
\[
\int_0^1 e^{e^x - x} \, dx = \int_1^e \frac{e^u}{u^2} \, du
\]
We integrate by parts, letting \(v = e^u\) and \(dw = \frac{du}{u^2}\). Then \(dv = e^u \, du\) and \(w = -\frac{1}{u}\). Applying integration by parts:
\[
\int \frac{e^u}{u^2} \, du = -\frac{e^u}{u} + \int \frac{e^u}{u} \, du = -\frac{e^u}{u} + \text{Ei}(u) + C
\]
Evaluating from \(u = 1\) to \(u = e\):
\[
\int_1^e \frac{e^u}{u^2} \, du = \left( -\frac{e^e}{e} + \text{Ei}(e) \right) - \left( -\frac{e^1}{1} + \text{Ei}(1) \right) = -\frac{e^e}{e} + \text{Ei}(e) + e - \text{Ei}(1)
\]

### Step 4: Combine the Results
Subtracting the second integral from the first:
\[
\left( \text{Ei}(e) - \text{Ei}(1) \right) - \left( -\frac{e^e}{e} + \text{Ei}(e) + e - \text{Ei}(1) \right)
\]
Simplifying, the \(\text{Ei}(e)\) and \(\text{Ei}(1)\) terms cancel, leaving:
\[
\frac{e^e}{e} - e = e^{e - 1} - e
\]

### Numerical Approximation
The exact result is \(e^{e - 1} - e\). Numerically, \(e \approx 2.718281828459045\), so \(e - 1 \approx 1.718281828459045\). Thus:
\[
e^{e - 1} \approx e^{1.718281828459045} \approx 5.7722587490
\]
Subtracting \(e\) gives:
\[
5.7722587490 - 2.7182818285 \approx 3.0539769205
\]

### Final Answer
The exact value is \(e^{e - 1} - e\), and the numerical approximation is approximately \(3.0539769205\).

{"answer": "e^{e - 1} - e", "numerical_answer": "3.0539769205"}