<think>
Okay, so I need to compute the definite integral of cos(x) divided by (1 + e^(-1/x)) from -1 to 1. Hmm, let me start by understanding the integrand. The function is cos(x)/(1 + e^(-1/x)). Wait, the denominator has an exponential term with 1/x. That might complicate things, especially around x=0 because as x approaches 0 from the positive side, 1/x goes to infinity, making e^(-1/x) approach 0. But from the negative side, as x approaches 0 from the left, 1/x is negative, so e^(-1/x) becomes e^(positive infinity), which blows up. So the denominator behaves differently on either side of zero.

First, let me check if the function is defined at x=0. When x approaches 0 from the right (x → 0+), 1/x → +∞, so e^(-1/x) → 0. Therefore, the denominator becomes 1 + 0 = 1, so the function approaches cos(0)/1 = 1. When x approaches 0 from the left (x → 0-), 1/x → -∞, so e^(-1/x) = e^(∞) → ∞. Therefore, the denominator becomes 1 + ∞, which is ∞, so the function approaches 0. So at x=0, the function has a jump discontinuity? Wait, the original function isn't defined at x=0 because 1/x is undefined there. So the integrand is undefined at x=0, but the integral is from -1 to 1. Hmm, so maybe this is an improper integral? Because the integrand has a discontinuity at x=0. So I need to split the integral into two parts: from -1 to 0 and from 0 to 1, taking limits as approaching 0 from the left and right.

But before that, maybe there's a symmetry or substitution that can simplify the problem. Let me think about substitution. Let me try substituting x = -t. Let’s see:

Let x = -t, so when x = -1, t = 1; when x = 1, t = -1. Then dx = -dt. So the integral becomes:

∫_{t=1}^{t=-1} [cos(-t)/(1 + e^(-1/(-t)))] (-dt) = ∫_{-1}^{1} [cos(t)/(1 + e^(1/t))] dt

Because cos(-t) = cos(t), and -1/(-t) = 1/t. So the integral from -1 to 1 of cos(x)/(1 + e^(-1/x)) dx is equal to the integral from -1 to 1 of cos(t)/(1 + e^(1/t)) dt. Let me write the original integral as I = ∫_{-1}^1 [cosx/(1 + e^{-1/x})] dx. Then, by substitution, I = ∫_{-1}^1 [cosx/(1 + e^{1/x})] dx.

Now, if I add the original integral I and the transformed integral, I get:

I + I = ∫_{-1}^1 [cosx/(1 + e^{-1/x}) + cosx/(1 + e^{1/x})] dx

Let me compute the sum inside the integral:

cosx/(1 + e^{-1/x}) + cosx/(1 + e^{1/x}) = cosx [1/(1 + e^{-1/x}) + 1/(1 + e^{1/x})]

Let’s compute the terms inside the brackets:

1/(1 + e^{-1/x}) + 1/(1 + e^{1/x}) = [1/(1 + e^{-1/x})] + [1/(1 + e^{1/x})]

Let me find a common denominator. Let’s denote y = 1/x for simplicity. Then the terms become 1/(1 + e^{-y}) + 1/(1 + e^{y}).

Multiply numerator and denominator of the first term by e^y:

= [e^y/(e^y + 1)] + [1/(1 + e^y)] = (e^y + 1)/(e^y + 1) = 1

So the sum of the two fractions is 1. Therefore, the integrand simplifies to cosx * 1 = cosx. Therefore, 2I = ∫_{-1}^1 cosx dx. Therefore, I = (1/2) ∫_{-1}^1 cosx dx.

That's a huge simplification! So the original integral is half the integral of cosx from -1 to 1. Let me compute that.

The integral of cosx is sinx. So ∫_{-1}^1 cosx dx = sin(1) - sin(-1) = sin(1) + sin(1) = 2 sin(1). Therefore, I = (1/2)(2 sin(1)) = sin(1).

So the exact answer is sin(1). Then the numerical approximation would be sin(1 radians). Let me compute that. Since 1 radian is approximately 57.3 degrees. The value of sin(1) is approximately 0.8414709848. Rounded to 10 decimal places, that's 0.8414709848. Let me check with a calculator. Yes, sin(1) ≈ 0.8414709848078965, so rounding to 10 decimal places gives 0.8414709848.

But let me verify the steps are correct. The key step was the substitution x = -t, leading to the transformed integral, and then adding them to get 2I equals the integral of cosx. That seems correct. Let me check the substitution again. When x is replaced by -t, the limits go from -1 to 1, which becomes t=1 to t=-1, and then reversing the limits cancels the negative sign from dx = -dt. So the transformed integral is indeed ∫_{-1}^1 cosx/(1 + e^{1/x}) dx. Then adding the original and transformed integrals gives the sum of cosx times [1/(1 + e^{-1/x}) + 1/(1 + e^{1/x})] which simplifies to cosx. Therefore, 2I = ∫_{-1}^1 cosx dx. That seems correct.

Therefore, the exact answer is sin(1), and the numerical approximation is approximately 0.8414709848.
</think>

{"answer": "\\sin(1)", "numerical_answer": "0.8414709848"}