We wish to evaluate
  I = ∫₀^(1/2) ln(√(1 – x) – √x) dx.
A useful method is to make the substitution

  x = sin²t   ⇒  dx = 2 sin t cos t dt,
  when x = 0 then t = 0 and when x = 1/2 then sin²t = 1/2 so that t = π/4.

In terms of t the square roots become
  √(1 – x) = cos t  and  √x = sin t.
Thus the integrand becomes
  ln( cos t – sin t ).
Also,
  2 sin t cos t = sin(2t).

So the integral becomes
  I = ∫₀^(π/4) sin(2t) ln( cos t – sin t ) dt.

A key observation is that we can rewrite the expression in the logarithm using the trigonometric identity
  cos t – sin t = √2 cos(t + π/4).
Then
  ln( cos t – sin t ) = ln(√2 cos(t + π/4)) = ln√2 + ln(cos(t + π/4))
             = (1/2) ln 2 + ln(cos(t + π/4)).

Thus the integral splits into two parts:
  I = ∫₀^(π/4) sin(2t)[ (1/2) ln 2 + ln(cos(t + π/4)) ] dt
    = (1/2 ln2) ∫₀^(π/4) sin(2t) dt + ∫₀^(π/4) sin(2t) ln(cos(t + π/4)) dt.

We first compute
  A = ∫₀^(π/4) sin(2t) dt.
An antiderivative is –cos(2t)/2 so that
  A = [–cos(2t)/2]₀^(π/4) = [–cos(π/2) + cos(0)]/2 = (0 + 1)/2 = 1/2.
Thus the first part is
  (1/2 ln2) · (1/2) = (1/4) ln2.

Now define the second part as
  B = ∫₀^(π/4) sin(2t) ln(cos(t + π/4)) dt.
Make the substitution
  u = t + π/4  ⇒  du = dt.
When t = 0, then u = π/4; when t = π/4, u = π/2.
Also, note that
  sin(2t) = sin(2(u – π/4)) = sin(2u – π/2).
Recalling the identity sin(θ – π/2) = –cos θ we have
  sin(2u – π/2) = –cos(2u).
Thus
  B = ∫(u = π/4)^(π/2) [–cos(2u)] ln(cos u) du = –∫(π/4)^(π/2) cos(2u) ln(cos u) du.
Call this last integral
  L = ∫(π/4)^(π/2) cos(2u) ln(cos u) du,
so that
  B = –L.

To compute L we use integration by parts. Write
  w = ln(cos u)  ⇒  dw = –tan u du,
  dv = cos(2u) du  ⇒  v = ∫cos(2u) du = (1/2) sin(2u).
Then
  L = [w·v]_(π/4)^(π/2) – ∫_(π/4)^(π/2) v dw
     = [ (ln(cos u)) (sin(2u)/2) ]_(π/4)^(π/2) – ∫_(π/4)^(π/2) (sin(2u)/2)(–tan u) du.
We now deal with the boundary term and the remaining integral.

• Boundary term:
 At u = π/2, cos(π/2) = 0 so ln(cos(π/2)) tends to –∞. However, sin(2u) at u = π/2 gives sin(π) = 0, and a careful limit shows that the product tends to 0.
 At u = π/4, cos(π/4) = √2/2 so ln(cos(π/4)) = ln(√2/2) = –(1/2) ln2 and sin(2(π/4)) = sin(π/2) = 1.
 Thus the boundary term is
  [(0) – ((–(1/2 ln2)·(1/2)))] = ln2/4.

• The remaining integral:
 I₁ = ∫_(π/4)^(π/2) (sin(2u)/2)(–tan u) du = –(1/2) ∫_(π/4)^(π/2) sin(2u) tan u du.
Notice that
 tan u = sin u/cos u  and  sin(2u) = 2 sin u cos u,
so that
 sin(2u) tan u = 2 sin u cos u · (sin u/cos u) = 2 sin²u.
Thus,
 I₁ = –(1/2) ∫_(π/4)^(π/2) 2 sin²u du = –∫_(π/4)^(π/2) sin²u du.
We know that
 ∫ sin²u du = (u/2 – sin(2u)/4) + C.
So, evaluating from u = π/4 to u = π/2:
 At u = π/2: (π/2)/2 – sin(π)/4 = π/4.
 At u = π/4: (π/4)/2 – sin(π/2)/4 = π/8 – 1/4.
Thus,
 ∫_(π/4)^(π/2) sin²u du = (π/4) – (π/8 – 1/4) = π/8 + 1/4.
So the remaining integral gives
 I₁ = – (π/8 + 1/4).

Altogether, the integration by parts gives:
 L = [boundary] – [I₁] = (ln2/4) – [–(π/8 + 1/4)] = ln2/4 + π/8 + 1/4.

Recall that B = –L so that
 B = –(ln2/4 + π/8 + 1/4).

Now we go back to our original splitting:
 I = (1/4 ln2) + B = (1/4 ln2) – (ln2/4 + π/8 + 1/4) = – (π/8 + 1/4).

Thus, the exact answer is
  I = – (π + 2) / 8.

Finally, for a numerical approximation:
 π + 2 ≈ 3.1415926536 + 2 = 5.1415926536,
 so I ≈ – (5.1415926536/8) ≈ –0.6426990817.

The final answer in JSON format is:
{"answer": "-\\frac{\\pi+2}{8}", "numerical_answer": "-0.6426990817"}