<think>
Okay, so I need to compute the definite integral from 0 to 2 of x^(1/2) times (2 - x)^(-1/2) times cosh of the square root of x(2 - x) dx. Hmm, let's start by understanding the integral.

First, the integrand is x^(1/2) * (2 - x)^(-1/2) * cosh(sqrt(x(2 - x))). The limits are from 0 to 2. Maybe a substitution would help here. Let me think about possible substitutions.

The expression inside the cosh is sqrt(x(2 - x)). Let me denote that as some variable. Let's say t = sqrt(x(2 - x)). But maybe a substitution would complicate things. Alternatively, perhaps a trigonometric substitution? Since the term x(2 - x) resembles a quadratic that can be rewritten as 1 - (x - 1)^2 if we complete the square. Let me check:

x(2 - x) = 2x - x^2 = -x^2 + 2x = -(x^2 - 2x) = -(x^2 - 2x +1 -1) = -(x -1)^2 +1. So, x(2 - x) = 1 - (x -1)^2. So sqrt(x(2 - x)) = sqrt(1 - (x -1)^2). That looks like the equation of a semicircle with radius 1 centered at x=1. So maybe a substitution like u = x -1? Let me try that.

Let u = x -1. Then x = u +1, and when x=0, u=-1; x=2, u=1. The integral becomes from u=-1 to u=1. Let's substitute:

x = u +1, so dx = du. The integrand becomes (u +1)^(1/2) * (2 - (u +1))^(-1/2) * cosh(sqrt{(u +1)(1 - u)}).

Simplify the terms:

2 - (u +1) = 1 - u. So (2 - x)^(-1/2) becomes (1 - u)^(-1/2). The term inside the cosh is sqrt{(u +1)(1 - u)} = sqrt{1 - u^2}. So the integrand is (u +1)^(1/2) * (1 - u)^(-1/2) * cosh(sqrt{1 - u^2}).

Hmm, that's a bit better. Let me write that:

Integral from u=-1 to u=1 of (u +1)^(1/2) * (1 - u)^(-1/2) * cosh(sqrt{1 - u^2}) du.

Hmm, maybe another substitution. Let's consider t = sqrt{1 - u^2}. Then t = sqrt{1 - u^2}, so t^2 = 1 - u^2. Differentiating both sides, 2t dt = -2u du, so du = - (t dt)/u. But maybe that's not helpful. Alternatively, perhaps a trigonometric substitution here. Let me set u = sinθ. Then when u = -1, θ = -π/2; u=1, θ=π/2. Then du = cosθ dθ. Let's try that.

So substituting u = sinθ, then sqrt{1 - u^2} = cosθ. The integrand becomes:

(u +1)^(1/2) * (1 - u)^(-1/2) * cosh(cosθ) * cosθ dθ.

Wait, let's compute each part:

(u +1) = sinθ +1 = 1 + sinθ. So (1 + sinθ)^(1/2).

(1 - u)^(-1/2) = (1 - sinθ)^(-1/2).

So the integrand is [ (1 + sinθ)^(1/2) / (1 - sinθ)^(1/2) ) ] * cosh(cosθ) * cosθ dθ.

Simplify the fraction:

(1 + sinθ)/(1 - sinθ) all to the 1/2 power. Let's rationalize that. Multiply numerator and denominator by (1 + sinθ):

sqrt( (1 + sinθ)^2 / (1 - sin^2θ) ) = sqrt( (1 + sinθ)^2 / cos^2θ ) = (1 + sinθ)/cosθ.

But since we have sqrt[(1 + sinθ)/(1 - sinθ)] = sqrt( (1 + sinθ)^2 / (1 - sin^2θ) ) = (1 + sinθ)/|cosθ|. But since θ is between -π/2 and π/2, cosθ is non-negative, so |cosθ| = cosθ. Therefore, the fraction simplifies to (1 + sinθ)/cosθ. Therefore, the integrand becomes:

sqrt( (1 + sinθ)/(1 - sinθ) ) * cosh(cosθ) * cosθ dθ = [ (1 + sinθ)/cosθ ]^(1/2) * cosh(cosθ) * cosθ dθ.

Wait, but sqrt( (1 + sinθ)/(1 - sinθ) ) is (1 + sinθ)/cosθ, as we saw. So multiplying by cosθ gives (1 + sinθ)/cosθ * cosθ = 1 + sinθ. Wait, no:

Wait, the original integrand after substitution is:

[ (1 + sinθ)^(1/2) / (1 - sinθ)^(1/2) ) ] * cosh(cosθ) * cosθ dθ.

Which is equal to sqrt( (1 + sinθ)/(1 - sinθ) ) * cosh(cosθ) * cosθ dθ.

But sqrt( (1 + sinθ)/(1 - sinθ) ) is (1 + sinθ)/sqrt(1 - sin^2θ) ) = (1 + sinθ)/cosθ. Therefore, the integrand becomes:

(1 + sinθ)/cosθ * cosh(cosθ) * cosθ dθ = (1 + sinθ) * cosh(cosθ) dθ.

Wait, the cosθ in the denominator cancels with the cosθ from the substitution. So we have (1 + sinθ) * cosh(cosθ) dθ. Therefore, the integral becomes:

Integral from θ = -π/2 to θ = π/2 of (1 + sinθ) * cosh(cosθ) dθ.

Hmm, that seems more manageable. Let's split the integral into two parts:

Integral of cosh(cosθ) dθ + Integral of sinθ * cosh(cosθ) dθ, both from -π/2 to π/2.

Let's consider the first integral: I1 = ∫_{-π/2}^{π/2} cosh(cosθ) dθ.

The second integral: I2 = ∫_{-π/2}^{π/2} sinθ * cosh(cosθ) dθ.

Let's evaluate I2 first. Notice that the integrand of I2 is sinθ * cosh(cosθ). Let's make a substitution here. Let’s set u = cosθ. Then du = -sinθ dθ. When θ = -π/2, u = 0; θ = π/2, u = 0. Wait, but integrating from θ=-π/2 to π/2 would translate to u from 0 to 0. So the integral becomes:

I2 = ∫_{u=0}^{0} - cosh(u) du = 0. Therefore, the integral I2 is zero. Because the limits are the same. So that term drops out.

Therefore, the original integral reduces to I1 = ∫_{-π/2}^{π/2} cosh(cosθ) dθ.

But since cosh(cosθ) is an even function (cosh is even, cosθ is even, so composition is even), and the interval is symmetric around 0, we can write this as 2 * ∫_{0}^{π/2} cosh(cosθ) dθ.

Wait, but wait, the original substitution was u = sinθ, leading to θ from -π/2 to π/2. But after substitution, we have I1 as the integral from -π/2 to π/2 of cosh(cosθ) dθ. Since cosh(cosθ) is even, this is 2 * integral from 0 to π/2 of cosh(cosθ) dθ.

But how do we compute this integral? The integral of cosh(cosθ) dθ from 0 to π/2. Hmm, this seems non-trivial. Let me recall that integrals involving cosh(cosθ) might relate to Bessel functions or modified Bessel functions. Let me check.

The modified Bessel function of the first kind, I_n(x), has integral representations. For example, I_0(z) = (1/π) ∫_{0}^{π} e^{z cosθ} dθ. Similarly, integrating cosh(z cosθ) would relate to I_0(z). Let me verify.

We know that cosh(z cosθ) = [e^{z cosθ} + e^{-z cosθ}]/2. So integrating from 0 to π:

∫_{0}^{π} cosh(z cosθ) dθ = (1/2)[∫_{0}^{π} e^{z cosθ} dθ + ∫_{0}^{π} e^{-z cosθ} dθ ].

But since cosθ is symmetric around θ=π/2, the integral from 0 to π of e^{z cosθ} dθ is the same as the integral from 0 to π of e^{-z cosθ} dθ. Therefore, this becomes ∫_{0}^{π} e^{z cosθ} dθ. Therefore, ∫_{0}^{π} cosh(z cosθ) dθ = ∫_{0}^{π} e^{z cosθ} dθ. But according to the definition, I_0(z) = (1/π) ∫_{0}^{π} e^{z cosθ} dθ. Therefore, ∫_{0}^{π} cosh(z cosθ) dθ = π I_0(z).

But in our case, the integral is from 0 to π/2 of cosh(cosθ) dθ. Let me see. Let’s set z=1 here. So if we have ∫_{0}^{π} cosh(cosθ) dθ = π I_0(1). But we need ∫_{0}^{π/2} cosh(cosθ) dθ. Hmm, perhaps we can express this in terms of I_0(1).

Alternatively, note that ∫_{0}^{π/2} cosh(cosθ) dθ = (1/2) ∫_{0}^{π} cosh(cosθ) dθ, because cosh(cosθ) is symmetric around θ=π/2. Wait, is that true? Let me check.

For θ in [0, π], cosθ is symmetric around θ=π/2. So cos(π - θ) = -cosθ. But cosh is even, so cosh(cos(π - θ)) = cosh(-cosθ) = cosh(cosθ). Therefore, the function cosh(cosθ) is symmetric around θ=π/2. Therefore, the integral from 0 to π is twice the integral from 0 to π/2. Therefore, ∫_{0}^{π/2} cosh(cosθ) dθ = (1/2) ∫_{0}^{π} cosh(cosθ) dθ = (1/2) * π I_0(1) = (π/2) I_0(1).

Therefore, our integral I1, which is 2 * ∫_{0}^{π/2} cosh(cosθ) dθ, becomes 2 * (π/2) I_0(1) = π I_0(1).

So the original integral is equal to π I_0(1), where I_0 is the modified Bessel function of the first kind of order 0.

Therefore, the exact answer is π times I_0(1). Now, we need to express this in terms of known functions or constants, but I_0(1) is a standard special function. So the analytical solution is π I_0(1).

But let me confirm the steps again to make sure. Starting from the original integral, substitution u = x -1, then trigonometric substitution u = sinθ, leading to the integral in terms of θ, splitting into two integrals, one of which is zero, and the other reduces to 2 times the integral from 0 to π/2 of cosh(cosθ) dθ, which is π I_0(1). That seems correct.

Now, the problem asks for the exact answer, which is π I_0(1). However, sometimes integrals can be expressed in terms of elementary functions, but in this case, since the integral involves cosh(cosθ), which doesn't have an elementary antiderivative, the result in terms of the Bessel function is the exact answer.

Now, maybe there's another way to compute the original integral without going through the Bessel function. Let me think again. The original integral was ∫₀² x^{1/2} (2 - x)^{-1/2} cosh(√(x(2 - x))) dx.

Alternatively, perhaps another substitution. Let me try t = √(x(2 - x)). Then t^2 = x(2 - x). Let me see if this substitution helps. Let’s compute dt/dx:

dt/dx = [ (2 - x) + x*(-1) ] / (2√(x(2 - x))) ) = (2 - 2x)/(2t) = (1 - x)/t.

Hmm, not sure if that helps. Alternatively, maybe substitution y = x -1, but similar to before.

Alternatively, let's consider the substitution x = 2 sin²(θ/2). Wait, maybe a substitution that simplifies the square roots. Let me try x = 2 sin²φ. Then when x=0, φ=0; x=2, φ=π/2. Then dx = 4 sinφ cosφ dφ. Let's substitute:

x = 2 sin²φ, so sqrt(x) = sqrt(2) sinφ.

(2 - x) = 2 - 2 sin²φ = 2 cos²φ, so (2 - x)^(-1/2) = 1/(sqrt(2) cosφ).

sqrt(x(2 - x)) = sqrt(2 sin²φ * 2 cos²φ) = sqrt(4 sin²φ cos²φ) = 2 sinφ cosφ.

Therefore, cosh(sqrt(x(2 - x))) = cosh(2 sinφ cosφ) = cosh(sin(2φ)).

Putting it all together, the integrand becomes:

sqrt(2) sinφ * (1/(sqrt(2) cosφ)) * cosh(sin(2φ)) * 4 sinφ cosφ dφ.

Simplify:

sqrt(2) * 1/sqrt(2) = 1. Then:

sinφ / cosφ * 4 sinφ cosφ = 4 sin²φ.

So the integrand simplifies to 4 sin²φ * cosh(sin(2φ)) dφ.

So the integral becomes ∫ from φ=0 to φ=π/2 of 4 sin²φ cosh(sin(2φ)) dφ.

Hmm, not sure if this is better. Let's see. Maybe expanding cosh(sin(2φ)) in a Taylor series?

Cosh(z) = Σ_{n=0}^∞ z^{2n}/(2n)!.

So cosh(sin(2φ)) = Σ_{n=0}^∞ [sin^{2n}(2φ)]/(2n)!.

Then the integral becomes 4 Σ_{n=0}^∞ [1/(2n)!] ∫_{0}^{π/2} sin²φ sin^{2n}(2φ) dφ.

But integrating sin²φ sin^{2n}(2φ) dφ from 0 to π/2. This seems complicated. Maybe not helpful.

Alternatively, perhaps using substitution in this form. Let’s set t = 2φ. Then φ = t/2, dφ = dt/2. When φ=0, t=0; φ=π/2, t=π. Then the integral becomes:

4 ∫_{0}^{π} sin²(t/2) sin^{2n}(t) * (1/2) dt.

But this might not help. Alternatively, perhaps another substitution. Let me think.

Alternatively, perhaps integrating by parts. Let me consider the original integral after substitution x = 2 sin²φ. The integrand is 4 sin²φ cosh(sin(2φ)) dφ. Let’s set u = sin(2φ), but not sure.

Alternatively, note that sin(2φ) = 2 sinφ cosφ. So sin(2φ) = 2 sinφ cosφ. So maybe express the integrand in terms of sin(2φ). But I don't see an immediate simplification.

Alternatively, perhaps this substitution is not better than the previous one. Let's go back to the previous result where the integral is π I_0(1). Let me check if that's correct.

The modified Bessel function I_0(z) is given by:

I_0(z) = (1/π) ∫_{0}^{π} e^{z cosθ} dθ.

Therefore, ∫_{0}^{π} e^{z cosθ} dθ = π I_0(z).

Similarly, ∫_{0}^{π} cosh(z cosθ) dθ = π I_0(z), since cosh(z cosθ) = [e^{z cosθ} + e^{-z cosθ}]/2, but integrating over 0 to π would give the same as integrating e^{z cosθ} because of symmetry. Wait, no:

Wait, if we integrate cosh(z cosθ) from 0 to π, we have:

∫_{0}^{π} cosh(z cosθ) dθ = ∫_{0}^{π} [e^{z cosθ} + e^{-z cosθ}]/2 dθ = (1/2)[π I_0(z) + π I_0(-z)].

But since I_0(z) is even function (I_0(-z) = I_0(z)), this becomes (1/2)(π I_0(z) + π I_0(z)) = π I_0(z). So yes, ∫_{0}^{π} cosh(z cosθ) dθ = π I_0(z).

Therefore, in our case, z=1, so ∫_{0}^{π} cosh(cosθ) dθ = π I_0(1). Then, since the integral from 0 to π/2 is half of that, because of symmetry, ∫_{0}^{π/2} cosh(cosθ) dθ = (π/2) I_0(1). Therefore, the original integral I1, which is 2 times this, is π I_0(1). So the integral is π I_0(1).

Therefore, the exact answer is π times the modified Bessel function of the first kind of order 0 evaluated at 1. So in LaTeX, that's \pi I_0(1). But sometimes, the modified Bessel function is written with a subscript, so maybe \pi I_0(1).

Now, the problem also asks for a numerical approximation. The value of I_0(1) is known. Let me recall that I_0(1) ≈ 1.266065878. Let me verify this with a calculator or a table. For example, the modified Bessel function I_0(1) can be computed as the sum of the series:

I_0(1) = Σ_{k=0}^∞ (1/ (k! )^2 ) (1/2)^{2k} ) = Σ_{k=0}^\infty 1/( (k!)^2 4^k ) ).

But actually, the general series for I_0(z) is Σ_{k=0}^\infty ( (z/2)^{2k} ) / (k!)^2 ). So for z=1, it's Σ_{k=0}^\infty 1/( (k!)^2 4^k ). Let's compute a few terms:

k=0: 1/(1 * 1) = 1

k=1: 1/(1 * 4) = 0.25

k=2: 1/(4 * 16) = 1/64 ≈ 0.015625

k=3: 1/(36 * 64) ≈ 0.000434

k=4: 1/(576 * 256) ≈ 0.78125e-5

Adding these up: 1 + 0.25 = 1.25; +0.015625 = 1.265625; +0.000434 ≈ 1.266059; +0.0000078125 ≈ 1.266067. So up to k=4, we get approximately 1.266067. The actual value is approximately 1.266065877752578... So rounding to 10 decimal places, it's about 1.2660658778.

Therefore, π times this is approximately 3.1415926536 * 1.2660658778 ≈ let's compute that.

First, 1.2660658778 * 3 = 3.7981976334

1.2660658778 * 0.1415926536 ≈

Compute 1.2660658778 * 0.1 = 0.12660658778

1.2660658778 * 0.04 = 0.05064263511

1.2660658778 * 0.0015926536 ≈ approx:

First, 1.2660658778 * 0.001 = 0.00126606588

1.2660658778 * 0.0005 = 0.00063303294

1.2660658778 * 0.0000926536 ≈ approx 0.0001173

Adding these: 0.00126606588 + 0.00063303294 = 0.00189909882 + 0.0001173 ≈ 0.0020164.

So total for 0.1415926536 * 1.2660658778 ≈ 0.12660658778 + 0.05064263511 + 0.0020164 ≈ 0.1792656229.

Therefore, total π * I_0(1) ≈ 3.7981976334 + 0.1792656229 ≈ 3.9774632563.

But let's use a calculator for more precision. Alternatively, use known values. The value of I_0(1) is approximately 1.266065877752, so π times that is:

1.266065877752 * π ≈ 1.266065877752 * 3.141592653589793 ≈

Let me compute this step by step:

1.266065877752 * 3 = 3.798197633256

1.266065877752 * 0.141592653589793 ≈

Compute 1.266065877752 * 0.1 = 0.1266065877752

1.266065877752 * 0.04 = 0.05064263511008

1.266065877752 * 0.001592653589793 ≈

First, 1.266065877752 * 0.001 = 0.001266065877752

1.266065877752 * 0.0005 = 0.000633032938876

1.266065877752 * 0.000092653589793 ≈

Approximate:

0.000092653589793 * 1.266065877752 ≈

Let's compute 1.266065877752 * 0.00009 = 0.000113945929

And 1.266065877752 * 0.000002653589793 ≈ ~0.00000336

So total ≈ 0.000113945929 + 0.00000336 ≈ 0.000117306

So adding up:

0.001266065877752 + 0.000633032938876 ≈ 0.001899098816628

+0.000117306 ≈ 0.002016404816628

Now, adding the parts:

0.1266065877752 + 0.05064263511008 ≈ 0.17724922288528

+0.002016404816628 ≈ 0.1792656277019

So total π * I_0(1) ≈ 3.798197633256 + 0.1792656277019 ≈ 3.9774632609579.

Rounded to 10 decimal places, that's approximately 3.9774632610.

But let me check using a calculator. If I use a calculator, I_0(1) ≈ 1.266065877752, then π * 1.266065877752 ≈ 3.97746326095. So rounding to 10 decimal places, 3.97746326095 becomes 3.9774632610.

But let me verify with a more precise calculation. Alternatively, use a computational tool. However, since I don't have one here, I'll proceed with this approximation.

Therefore, the exact answer is π I_0(1), and the numerical approximation is approximately 3.9774632610.

So the final answer should be:

{"answer": "\\pi I_0(1)", "numerical_answer": "3.9774632610"}

But wait, the problem says to put the exact answer in LaTeX. The modified Bessel function is standard, so writing \pi I_0(1) is acceptable. Alternatively, if the problem expects a different form, but given the steps, this is the exact answer.
</think>

{"answer": "\\pi I_0(1)", "numerical_answer": "3.9774632610"}