Given:

\[
I = \int_{0}^{4} x^{-1/2} (4-x)^{-1/2} \left[1 - 0.25x(4-x)\right]^{1/2} dx
\]

Let's proceed step by step.

---

**Step 1: Substitution**

Let us use the substitution \( x = 4 \sin^2\theta \), with \( 0 \leq \theta \leq \pi/2 \).

Then:
- \( dx = 8 \sin\theta\cos\theta d\theta = 4\sin2\theta d\theta \)
- \( x^{-1/2} = (4\sin^2\theta)^{-1/2} = \frac{1}{2\sin\theta} \)
- \( 4-x = 4 - 4\sin^2\theta = 4\cos^2\theta \implies (4-x)^{-1/2} = \frac{1}{2\cos\theta} \)
- \( x(4-x) = 4\sin^2\theta \cdot 4\cos^2\theta = 16\sin^2\theta\cos^2\theta = 4\sin^2 2\theta \)
- \( 1 - 0.25 x(4-x) = 1 - 0.25 \times 4 \sin^2 2\theta = 1 - \sin^2 2\theta = \cos^2 2\theta \)
- \( \sqrt{1 - 0.25 x(4-x)} = |\cos 2\theta| \), but for \( 0 \leq \theta \leq \frac{\pi}{2} \), \( \cos 2\theta \) goes from 1 to -1, so for \( \theta \in [0, \frac{\pi}{4}] \) it is non-negative, while for \( \theta \in [\frac{\pi}{4}, \frac{\pi}{2}] \) it is non-positive. Let's keep it as \( |\cos 2\theta| \).

---

Plug all into the integral:

\[
I = \int_{\theta=0}^{\theta=\pi/2} \frac{1}{2\sin\theta} \cdot \frac{1}{2\cos\theta} \cdot |\cos 2\theta| \cdot 4\sin2\theta d\theta
\]

Let's simplify coefficients:

\[
\frac{1}{2} \cdot \frac{1}{2} \cdot 4 = 1
\]

So,

\[
I = \int_0^{\pi/2} \frac{1}{\sin\theta\cos\theta} |\cos 2\theta| \sin2\theta d\theta
\]

But \( \sin2\theta = 2\sin\theta\cos\theta \), so:

\[
I = \int_0^{\pi/2} \frac{|\cos 2\theta| \cdot 2\sin\theta\cos\theta}{\sin\theta\cos\theta} d\theta = \int_0^{\pi/2} 2 |\cos 2\theta| d\theta
\]

So,

\[
I = 2 \int_0^{\pi/2} |\cos 2\theta| d\theta
\]

Let's split the integral at \(\theta = \frac{\pi}{4}\), since \( \cos 2\theta \) changes sign there.

- For \( 0 \leq \theta \leq \frac{\pi}{4} \): \( \cos 2\theta \geq 0 \), so \( |\cos 2\theta| = \cos 2\theta \)
- For \( \frac{\pi}{4} \leq \theta \leq \frac{\pi}{2} \): \( \cos 2\theta \leq 0 \), so \( |\cos 2\theta| = -\cos 2\theta \)

So we write:

\[
I = 2 \left( \int_0^{\pi/4} \cos 2\theta d\theta + \int_{\pi/4}^{\pi/2} -\cos 2\theta d\theta \right)
\]

\[
= 2 \left( \int_0^{\pi/4} \cos 2\theta d\theta - \int_{\pi/4}^{\pi/2} \cos 2\theta d\theta \right)
\]

Compute each integral:

\[
\int \cos 2\theta d\theta = \frac{1}{2} \sin 2\theta
\]

So,

\[
\int_0^{\pi/4} \cos 2\theta d\theta = \frac{1}{2} [\sin 2\theta]_{0}^{\pi/4} = \frac{1}{2} (\sin (\pi/2) - \sin 0) = \frac{1}{2} (1-0) = \frac{1}{2}
\]

\[
\int_{\pi/4}^{\pi/2} \cos 2\theta d\theta = \frac{1}{2} [\sin 2\theta]_{\pi/4}^{\pi/2} = \frac{1}{2} ( \sin(\pi) - \sin(\pi/2) ) = \frac{1}{2}(0-1) = -\frac{1}{2}
\]

So,

\[
I = 2 \left( \frac{1}{2} - ( -\frac{1}{2} ) \right ) = 2 \left( 1 \right ) = 2
\]

---

**Step 2: Final (Exact) Answer**

\[
\boxed{I = 2}
\]

---

**Step 3: Numerical approximation**

\[
I \approx 2.0000000000
\]

---

**Step 4: Output the JSON**

```json
{"answer": "2", "numerical_answer": "2.0000000000"}
```