Let's solve the integral step by step:

\[
I = \int_e^{e^e} \frac{\log x \cdot \log(\log x)}{x}\;dx
\]

**Step 1: Substitution**

Let’s use \( u = \log x \) (natural logarithm):

- When \( x = e \), \( u = 1 \).
- When \( x = e^e \), \( u = e \).
- \( dx = e^u du = x du \Rightarrow du = \frac{dx}{x} \).

Thus,
\[
I = \int_{u=1}^{u=e} u \cdot \log u \; du
\]

**Step 2: Integrate \( u \log u \)**

Let’s use integration by parts:

Let
- \( v = \log u \implies dv = \frac{1}{u} du \)
- \( w' = u \implies w = \frac{u^2}{2} \)

By parts:
\[
\int u \log u\; du = \frac{u^2}{2} \log u - \int \frac{u^2}{2} \cdot \frac{1}{u} du = \frac{u^2}{2} \log u - \frac{1}{2}\int u \, du = \frac{u^2}{2} \log u - \frac{1}{4}u^2 + C
\]

**Step 3: Apply the limits**

Apply from \( u = 1 \) to \( u = e \):

\[
I = \left[ \frac{u^2}{2} \log u - \frac{1}{4} u^2 \right]_{u=1}^{u=e}
\]

At \( u = e \):

- \( \log u = 1 \), \( u^2 = e^2 \)
- \( \frac{e^2}{2} \ log e - \frac{1}{4}e^2 = \frac{e^2}{2} \cdot 1 - \frac{e^2}{4} = \frac{e^2}{2} - \frac{e^2}{4} = \frac{e^2}{4} \)

At \( u = 1 \):

- \( \log u = 0 \), \( u^2 = 1 \)
- \( \frac{1}{2}\cdot 0 - \frac{1}{4} \cdot 1 = -\frac{1}{4} \)

So the definite integral is:

\[
I = \frac{e^2}{4} - \left( -\frac{1}{4} \right) = \frac{e^2}{4} + \frac{1}{4} = \frac{e^2 + 1}{4}
\]

**Step 4: Numerical approximation**

\( e \approx 2.7182818285 \Rightarrow e^2 \approx 7.3890560989 \)

So,

\[
I \approx \frac{7.3890560989 + 1}{4} = \frac{8.3890560989}{4} \approx 2.0972640247
\]

**Final Output (JSON):**
```json
{"answer": "\\frac{e^2+1}{4}", "numerical_answer": "2.0972640247"}
```