Let
\[
I = \int_0^\pi \sec x \ln\left(1 + \frac{\cos x}{3}\right) dx
\]

## 1. Symmetry and substitution

Let us consider the substitution \( x \to \pi - x \):

- \( \cos(\pi - x) = -\cos x \)
- \( \sec(\pi - x) = -\sec x \)

Thus,
\[
\begin{align*}
I &= \int_0^\pi \sec x \ln\left(1 + \frac{\cos x}{3}\right) dx \\
  &= \int_0^\pi \sec(\pi - x) \ln\left(1 + \frac{\cos(\pi - x)}{3}\right) dx \\
  &= \int_0^\pi \left[ -\sec x \right] \ln\left(1 - \frac{\cos x}{3}\right) dx \\
  &= -\int_0^\pi \sec x \ln\left(1 - \frac{\cos x}{3}\right) dx \\
\end{align*}
\]

Now, writing the sum of the original and transformed integrals:

\[
I + I = \int_0^\pi \sec x \left( \ln\left(1 + \frac{\cos x}{3}\right) + \ln\left(1 - \frac{\cos x}{3}\right) \right) dx
\]
\[
2I = \int_0^\pi \sec x \ln\left(1 - \frac{\cos^2 x}{9}\right) dx
\]

Thus,
\[
I = \frac{1}{2} \int_0^\pi \sec x \ln\left(1 - \frac{\cos^2 x}{9}\right) dx
\]

Since \(\sec x = \frac{1}{\cos x}\), substitute \(u = \cos x\) for \(x \in [0, \pi]\):

- When \(x = 0\), \(u = 1\)
- When \(x = \pi\), \(u = -1\)
- \(du = -\sin x\,dx\), so \(dx = -\frac{du}{\sin x}\)
- Note that \(\sin^2 x = 1 - \cos^2 x = 1 - u^2\)
- Thus, \(\sin x = \sqrt{1 - u^2}\) (positive for \(x \in (0,\pi)\))

Moreover,
\[
\sec x = \frac{1}{u}
\]
and
\[
dx = -\frac{du}{\sqrt{1-u^2}}
\]

Substituting all, we get:
\[
I = \frac{1}{2} \int_{x=0}^{x=\pi} \frac{1}{\cos x} \ln\left(1 - \frac{\cos^2 x}{9}\right) dx
= \frac{1}{2} \int_{u=1}^{u=-1} \frac{1}{u} \ln\left(1 - \frac{u^2}{9}\right) \left(-\frac{du}{\sqrt{1-u^2}}\right)
\]
\[
= -\frac{1}{2} \int_{u=1}^{u=-1} \frac{1}{u} \ln\left(1 - \frac{u^2}{9}\right) \frac{du}{\sqrt{1-u^2}}
\]
\[
= \frac{1}{2} \int_{u=-1}^{u=1} \frac{1}{u} \ln\left(1 - \frac{u^2}{9}\right) \frac{du}{\sqrt{1-u^2}}
\]

Let us split the integral into even and odd parts:

- \(\frac{1}{u}\) is odd in \(u\)
- \(\ln\left(1 - \frac{u^2}{9}\right)\) is even in \(u\)
- \(\frac{1}{\sqrt{1-u^2}}\) is even in \(u\)

Thus, integrand is odd (\(f(-u) = -f(u)\)), and integrating an odd function from \(-a\) to \(a\) gives 0, **except at the singularity at \(u=0\)**.

However, let us examine more closely: at \(u=0\), the integrand behaves like \(\frac{1}{u} \cdot \mathcal{O}(u^2)\), so the singularity at \(u=0\) is removable (since \(\ln(1-u^2/9)/u \sim -u/9\) as \(u \to 0\)), thus the principal value is well-defined and the integral is 0.

Thus,
\[
I = 0
\]

## 2. Steps summary

1. Used a substitution \(x \to \pi-x\) to simplify the integral.
2. Added the original and reflected integrals, obtaining a new integrand.
3. Used the substitution \(u = \cos x\) to change limits and variables.
4. Observed the integrand is odd over a symmetric interval, leading to an answer of 0.

## 3. Numerical approximation

\[
\boxed{0.0000000000}
\]

## 4. Final JSON answer

```json
{"answer": "0", "numerical_answer": "0.0000000000"}
```