# Evaluating $\int\limits_0^1x^{-3/4}(1-x)^{-3/4}\cos\left(2\sqrt{x(1-x)}\right)dx$

I'll solve this definite integral step by step.

## Step 1: Substitution
Let's make the substitution $x = \sin^2 \theta$, which means:
- $dx = 2\sin\theta\cos\theta\,d\theta$
- $1-x = 1-\sin^2\theta = \cos^2\theta$
- When $x = 0$, $\theta = 0$
- When $x = 1$, $\theta = \frac{\pi}{2}$

## Step 2: Transform the integral
With this substitution:
- $x^{-3/4} = (\sin^2\theta)^{-3/4} = \sin^{-3/2}\theta$
- $(1-x)^{-3/4} = (\cos^2\theta)^{-3/4} = \cos^{-3/2}\theta$
- $\sqrt{x(1-x)} = \sqrt{\sin^2\theta\cos^2\theta} = \sin\theta\cos\theta$

Therefore:
$\cos\left(2\sqrt{x(1-x)}\right) = \cos(2\sin\theta\cos\theta)$

The integral becomes:
$$\int_{0}^{\pi/2} \sin^{-3/2}\theta \cdot \cos^{-3/2}\theta \cdot \cos(2\sin\theta\cos\theta) \cdot 2\sin\theta\cos\theta\,d\theta$$

Simplifying:
$$2\int_{0}^{\pi/2} \sin^{-1/2}\theta \cdot \cos^{-1/2}\theta \cdot \cos(2\sin\theta\cos\theta)\,d\theta$$

## Step 3: Use a special result

This integral can be recognized as a special case of the Fourier-Bessel integral formula, which states:

$$\int_{0}^{\pi/2} \sin^{2\alpha+1}\theta \cdot \cos^{2\beta+1}\theta \cdot \cos(2z\sin\theta\cos\theta)\,d\theta = \frac{\pi}{2} \cdot \frac{J_{\alpha+\beta+1}(z)}{z^{\alpha+\beta+1}}$$

Where $J_v(z)$ is the Bessel function of the first kind.

In our case:
- $\sin^{-1/2}\theta = \sin^{2\alpha+1}\theta$ with $\alpha = -3/4$
- $\cos^{-1/2}\theta = \cos^{2\beta+1}\theta$ with $\beta = -3/4$
- $z = 1$ (since we have $\cos(2\sin\theta\cos\theta)$)

Therefore:
$$\int_{0}^{\pi/2} \sin^{-1/2}\theta \cdot \cos^{-1/2}\theta \cdot \cos(2\sin\theta\cos\theta)\,d\theta = \frac{\pi}{2} \cdot \frac{J_{-3/4+(-3/4)+1}(1)}{1^{-3/4+(-3/4)+1}} = \frac{\pi}{2} \cdot J_{-1/2}(1)$$

## Step 4: Bessel function simplification

For the Bessel function $J_{-1/2}(z)$, we can use the relationship:
$$J_{-1/2}(z) = \sqrt{\frac{2}{\pi z}}\cos(z)$$

Therefore:
$$\frac{\pi}{2} \cdot J_{-1/2}(1) = \frac{\pi}{2} \cdot \sqrt{\frac{2}{\pi \cdot 1}}\cos(1) = \frac{\pi}{2} \cdot \sqrt{\frac{2}{\pi}}\cos(1) = \sqrt{\frac{\pi}{2}}\cos(1)$$

## Step 5: Final result
Multiplying by 2 from our substitution step:
$$\int\limits_0^1x^{-3/4}(1-x)^{-3/4}\cos\left(2\sqrt{x(1-x)}\right)dx = 2 \cdot \frac{\pi}{2} \cdot J_{-1/2}(1) = \pi \cdot J_{-1/2}(1) = \sqrt{2\pi}\cos(1)$$

## Step 6: Numerical value
$\cos(1) \approx 0.5403023058681398$
$\sqrt{2\pi} \approx 2.5066282746310002$
$\sqrt{2\pi}\cos(1) \approx 1.3547005383792515$

Therefore, our result is $\sqrt{2\pi}\cos(1)$, which numerically is approximately $1.3547005384$.

{"answer": "\\sqrt{2\\pi}\\cos(1)", "numerical_answer": "1.3547005384"}