We start with the integral

  I = ∫₀ᴨ cos(x + cos x) dx.

Step 1. Symmetry transformation:
Make the substitution u = π - x. Then, when x = 0, u = π and when x = π, u = 0 with dx = –du. The integral becomes

  I = ∫₀ᴨ cos((π - u) + cos(π - u)) du.

Using the identity cos(π - u) = −cos u, notice that

  cos((π - u) + cos(π - u)) = cos((π - u) - cos u) 
               = cos(π - (u + cos u)).

Recalling that cos(π - θ) = -cos θ, we have

  cos(π - (u + cos u)) = -cos(u + cos u).

Therefore, the transformed integral is

  I = ∫₀ᴨ [−cos(u + cos u)] du = −∫₀ᴨ cos(u + cos u) du = −I.

Step 2. Conclude the evaluation:
We have I = −I, which implies

  2I = 0  ⟹  I = 0.

Thus the exact answer is 0.

Step 3. Numerical approximation:
Since the exact value is 0, its numerical approximation is also 0.0000000000 when rounded to 10 decimal places.

{"answer": "$0$", "numerical_answer": "0.0000000000"}