We start with the integral

  I = ∫₀¹ (ln(1 + x + x²) / x) dx.

Step 1. Express the integrand in a more useful form.

Notice that
  1 + x + x² = (x³ – 1)/(x – 1),  (for x ≠ 1).

Since for x in (0, 1) we have
  x³ – 1 = –(1 – x³)  and  x – 1 = –(1 – x),
we can write
  1 + x + x² = (1 – x³)/(1 – x).

Taking logarithms we obtain
  ln(1 + x + x²) = ln(1 – x³) – ln(1 – x).

Thus, the integral becomes
  I = ∫₀¹ [ln(1 – x³) – ln(1 – x)]/x dx
    = ∫₀¹ (ln(1 – x³)/x) dx – ∫₀¹ (ln(1 – x)/x) dx.

Step 2. Expand the logarithms into series.

Recall the Taylor series (for |x| < 1):
  ln(1 – u) = – Σₙ₌₁∞ uⁿ/n.

For the first term, set u = x³:
  ln(1 – x³) = – Σₙ₌₁∞ x^(3n)/n.

Hence,
  ∫₀¹ (ln(1 – x³)/x) dx = – Σₙ₌₁∞ (1/n) ∫₀¹ x^(3n – 1) dx.
The integral ∫₀¹ x^(3n – 1) dx is 1/(3n). Thus we get
  ∫₀¹ (ln(1 – x³)/x) dx = – Σₙ₌₁∞ 1/(n·3n) = – (1/3) Σₙ₌₁∞ 1/n²
    = – (1/3) ζ(2).

Similarly, for the second term, set u = x:
  ln(1 – x) = – Σₙ₌₁∞ xⁿ/n.
Then
  ∫₀¹ (ln(1 – x)/x) dx = – Σₙ₌₁∞ (1/n) ∫₀¹ x^(n – 1) dx = – Σₙ₌₁∞ 1/(n²)
    = – ζ(2).

Step 3. Combine the results.

We have
  I = [– (1/3) ζ(2)] – [– ζ(2)] = ζ(2) – (1/3) ζ(2) = (2/3) ζ(2).

It is known that ζ(2) = π²/6, so
  I = (2/3) (π²/6) = π²/9.

Step 4. Provide the numerical approximation.

Using π² ≈ 9.869604401089358, we find
  I ≈ 9.869604401089358/9 ≈ 1.096622711232151,
which rounded to 10 decimal places is 1.0966227112.

The final answer in the required JSON format is:
{"answer": "\\frac{\\pi^2}{9}", "numerical_answer": "1.0966227112"}