Let’s compute the integral:
\[
I = \int_{0}^{\infty}\frac{x^{3}}{e^x-1}\left[8\cosh\left(0.5x\right)-\cosh\left(0.25x\right)\right]dx
\]

Let us analyze the structure:

Recall that \(\cosh(ax) = \frac{e^{ax} + e^{-ax}}{2}\), so:
\[
8\cosh(0.5x) - \cosh(0.25x) = 8 \frac{e^{0.5x} + e^{-0.5x}}{2} - \frac{e^{0.25x} + e^{-0.25x}}{2}
= 4(e^{0.5x} + e^{-0.5x}) - \frac{1}{2}(e^{0.25x} + e^{-0.25x})
\]
\[
= 4e^{0.5x} + 4e^{-0.5x} - \frac{1}{2}e^{0.25x} - \frac{1}{2}e^{-0.25x}
\]

Thus, the integral becomes:
\[
I = \int_0^\infty \frac{x^3}{e^x-1} \left(4e^{0.5x} + 4e^{-0.5x} - \frac{1}{2}e^{0.25x} - \frac{1}{2}e^{-0.25x}\right) dx
\]
\[
= 4 \int_0^\infty \frac{x^3 e^{0.5x}}{e^x-1}dx + 4 \int_0^\infty \frac{x^3 e^{-0.5x}}{e^x-1}dx
- \frac{1}{2}\int_0^\infty \frac{x^3 e^{0.25x}}{e^x-1}dx - \frac{1}{2}\int_0^\infty \frac{x^3 e^{-0.25x}}{e^x-1}dx
\]

Let’s analyze the general term:
\[
J(a) = \int_0^\infty \frac{x^3 e^{a x}}{e^x-1} dx,\qquad a\in \mathbb{R}
\]

We expand \( \frac{1}{e^x - 1} = \sum_{n=1}^\infty e^{-n x} \); so,
\[
\frac{x^3 e^{a x}}{e^x-1} = x^3 e^{a x} \sum_{n=1}^\infty e^{-n x} 
= \sum_{n=1}^\infty x^3 e^{(a - n)x}
\]

Thus,
\[
J(a) = \sum_{n=1}^\infty \int_0^\infty x^3 e^{(a-n)x} dx
\]

The integral is (for \(p < 0\)): \(\int_0^\infty x^k e^{p x} dx = \frac{k!}{(-p)^{k+1}}\)

So for \(n > a\), \((a-n)<0\),
\[
\int_0^\infty x^3 e^{(a-n)x} dx = \frac{3!}{(n-a)^4}
= \frac{6}{(n-a)^4}
\]

Therefore,
\[
J(a) = \sum_{n=1}^\infty \frac{6}{(n-a)^4}
= 6\sum_{n=1}^\infty \frac{1}{(n-a)^4}
\]

Recall the definition of the Hurwitz zeta function:
\[
\zeta(s, q) = \sum_{n=0}^\infty \frac{1}{(n+q)^s}
\]
We can relate
\[
\sum_{n=1}^\infty \frac{1}{(n-a)^4} 
= \zeta(4, 1-a)
\]

So,
\[
J(a) = 6\zeta(4, 1-a)
\]

Now, back to our integral:
\[
I = 4J(0.5) + 4J(-0.5) - \frac{1}{2}J(0.25) - \frac{1}{2}J(-0.25)
\]

Thus,
\[
I = 24\zeta(4, 0.5) + 24\zeta(4, 1.5) - 3\zeta(4, 0.75) - 3\zeta(4, 1.25)
\]

But, since
\[
\zeta(4, q) = \sum_{n=0}^\infty \frac{1}{(n+q)^4}
\]
and
\[
\zeta(4, 1-q) = \sum_{n=0}^\infty \frac{1}{(n+1-q)^4}
\]
So:
- \(\zeta(4, 0.5) = \sum_{n=0}^\infty \frac{1}{(n+0.5)^4}\)
- \(\zeta(4, 1.5) = \sum_{n=0}^\infty \frac{1}{(n+1.5)^4}\)
- etc.

Let’s see if we can further simplify. There’s a useful identity for positive integer \(m\):
\[
\zeta(s, 1 - q) + (-1)^s \zeta(s, q)
\]
For \(s = 4\) (even), the sums can sometimes combine.

However, more usefully, we could recall:
\[
\sum_{n=1}^\infty \frac{1}{n^4} = \zeta(4) = \frac{\pi^4}{90}
\]
And:
\[
\zeta(4, q) = \frac{1}{6} \frac{\partial^3}{\partial q^3} \zeta(1, q)
\]
But it may be faster, for our purposes, to use the known closed forms for certain arguments:

- For half-integer and quarter-integer arguments, there exist relations between Hurwitz zeta values and the usual Riemann zeta at integer arguments.

Let’s look up or recall these, or we can relate them to polygamma functions:
\[
\zeta(s,q) = \frac{(-1)^s}{\Gamma(s)} \psi^{(s-1)}(q)
\]
For \(s = 4\):
\[
\zeta(4, q) = \frac{1}{6} \psi^{(3)}(q)
\]

Thus,
\[
I = 24 \zeta(4, 0.5) + 24 \zeta(4, 1.5) - 3 \zeta(4, 0.75) - 3 \zeta(4, 1.25)
= 24 \cdot \frac{1}{6}\psi^{(3)}(0.5) + 24 \cdot \frac{1}{6}\psi^{(3)}(1.5) 
   - 3 \cdot \frac{1}{6}\psi^{(3)}(0.75) - 3 \cdot \frac{1}{6}\psi^{(3)}(1.25)
\]
\[
= 4 \psi^{(3)}(0.5) + 4 \psi^{(3)}(1.5) - 0.5 \psi^{(3)}(0.75) - 0.5 \psi^{(3)}(1.25)
\]

Now, recall the polygamma reflection and shift properties:
\[
\psi^{(n)}(1-z) + (-1)^{n+1} \psi^{(n)}(z) = \pi \frac{d^n}{dz^n} \cot \pi z
\]

For \(n=3\) (so even degree: \(n+1=4\) is even, so a + sign):
\[
\psi^{(3)}(1-z) + \psi^{(3)}(z) = \pi \frac{d^3}{dz^3} \cot \pi z
\]

But since \(\psi^{(3)}(1.5) = \psi^{(3)}(0.5)\), etc., so let's use shift:
\[
\psi^{(3)}(z+1) = \psi^{(3)}(z) - \frac{6}{z^4}
\]

So:
\[
\psi^{(3)}(1.5) = \psi^{(3)}(0.5) - \frac{6}{(0.5)^4} = \psi^{(3)}(0.5) - 96
\]
Similarly,
\[
\psi^{(3)}(1.25) = \psi^{(3)}(0.25) - \frac{6}{(0.25)^4} = \psi^{(3)}(0.25) - 1536
\]

But let's just write the value in terms of \(\psi^{(3)}\):

So,
\[
I = 4 \psi^{(3)}(0.5) + 4 \psi^{(3)}(1.5) - 0.5 \psi^{(3)}(0.75) - 0.5 \psi^{(3)}(1.25)
\]

Now, let's plug in the shift formula:
- \(\psi^{(3)}(1.5) = \psi^{(3)}(0.5) - 96\)
- \(\psi^{(3)}(1.25) = \psi^{(3)}(0.25) - 1536\)

So,
\[
I = 4 \psi^{(3)}(0.5) + 4 (\psi^{(3)}(0.5) - 96)
- 0.5 \psi^{(3)}(0.75)
- 0.5 (\psi^{(3)}(0.25) - 1536)
\]
\[
= 4 \psi^{(3)}(0.5) + 4 \psi^{(3)}(0.5) - 384 
- 0.5 \psi^{(3)}(0.75)
- 0.5 \psi^{(3)}(0.25) + 768
\]
\[
= 8 \psi^{(3)}(0.5)
- 0.5 \psi^{(3)}(0.75)
- 0.5 \psi^{(3)}(0.25)
+ 768 - 384
\]
\[
= 8 \psi^{(3)}(0.5)
- 0.5 [\psi^{(3)}(0.75) + \psi^{(3)}(0.25)]
+ 384
\]

Now, use the reflection formula:
\[
\psi^{(3)}(1-z) + \psi^{(3)}(z) = \pi \frac{d^3}{dz^3} \cot \pi z
\]

For \(z = 0.25\): \(1-0.25 = 0.75\)

So:
\[
\psi^{(3)}(0.75) + \psi^{(3)}(0.25) = \pi \frac{d^3}{dz^3} \cot(\pi z) \Big|_{z=0.25}
\]

Let’s compute \(\frac{d^3}{dz^3} \cot(\pi z)\) at \(z = 0.25\):

First, \(\cot(\pi z)\).
Take derivatives:

First derivative:
\[
\frac{d}{dz} \cot(\pi z) = -\pi \csc^2(\pi z)
\]

Second derivative:
\[
\frac{d^2}{dz^2} \cot(\pi z)
= -\pi \frac{d}{dz} \csc^2(\pi z)
= -\pi \cdot 2\csc^2(\pi z) \cdot (-\pi)\cot(\pi z)\csc(\pi z)
= 2\pi^2 \cot(\pi z) \csc^2(\pi z)
\]

Third derivative:
\[
\frac{d^3}{dz^3} \cot(\pi z)
= 2\pi^2 \frac{d}{dz} \left[\cot(\pi z) \csc^2(\pi z)\right]
\]
Use product rule:

\[
\frac{d}{dz} \left[ \cot(\pi z) \csc^2(\pi z) \right]
= \frac{d}{dz} \cot(\pi z) \cdot \csc^2(\pi z)
+ \cot(\pi z)\cdot \frac{d}{dz} \csc^2(\pi z)
\]
\[
= -\pi \csc^2(\pi z) \cdot \csc^2(\pi z)
+ \cot(\pi z) \cdot 2\csc^2(\pi z)\cdot (-\pi) \cot(\pi z)\csc(\pi z)
\]
\[
= -\pi \csc^4(\pi z)
- 2\pi \cot^2(\pi z) \csc^3(\pi z)
\]

Now, substitute:
\[
\frac{d^3}{dz^3} \cot(\pi z)
= 2\pi^2 \left[ -\pi \csc^4(\pi z)
- 2\pi \cot^2(\pi z) \csc^3(\pi z)
\right]
\]
\[
= -2\pi^3 \csc^4(\pi z)
- 4\pi^3 \cot^2(\pi z) \csc^3(\pi z)
\]

So, at \(z=0.25\), \(\pi z = \frac{\pi}{4}\):

\[
\csc(\pi/4) = \frac{1}{\sin(\pi/4)} = \frac{1}{\sqrt{2}/2} = \sqrt{2}
\]
\[
\cot(\pi/4) = 1
\]

Thus:

- \(\csc^3(\pi/4) = (\sqrt{2})^3 = 2^{3/2} = 2\sqrt{2}\)
- \(\csc^4(\pi/4) = (\sqrt{2})^4 = 4\)
- \(\cot^2(\pi/4) = 1\)

So, the expression:
\[
\frac{d^3}{dz^3} \cot(\pi z) \Big|_{z=0.25}
= -2\pi^3 \cdot 4
- 4\pi^3 \cdot 1 \cdot 2\sqrt{2}
= -8\pi^3 - 8\pi^3 \sqrt{2}
\]

Therefore,
\[
\psi^{(3)}(0.75) + \psi^{(3)}(0.25) = \pi \left(-8\pi^3 - 8\pi^3 \sqrt{2}\right)
= -8\pi^4 (1+\sqrt{2})
\]

Plug this into our formula:
\[
I = 8\psi^{(3)}(0.5) - 0.5 [\psi^{(3)}(0.75) + \psi^{(3)}(0.25)] + 384
\]
\[
= 8\psi^{(3)}(0.5) - 0.5 \cdot [-8\pi^4 (1+\sqrt{2})] + 384
\]
\[
= 8\psi^{(3)}(0.5) + 4\pi^4 (1+\sqrt{2}) + 384
\]

Now, let's find \(\psi^{(3)}(0.5)\).

From known formulas:

\[
\psi^{(n)}(z) = (-1)^{n+1} n! \sum_{k=0}^\infty \frac{1}{(z+k)^{n+1}}
\]

For \(n=3\), \(z=0.5\):
\[
\psi^{(3)}(0.5) = -3! \sum_{k=0}^\infty \frac{1}{(0.5+k)^4}
= -6 \sum_{k=0}^\infty \frac{1}{(k+0.5)^4}
\]

But, \(\sum_{k=0}^\infty \frac{1}{(k+0.5)^4} = \zeta(4, 0.5)\), for which there is a closed form:
\[
\zeta(4, 0.5) = 16\zeta(4)
\]
(see e.g. https://functions.wolfram.com/ZetaFunctionsandPolylogarithms/Zeta2/03/01/03/0008/)

So,
\[
\psi^{(3)}(0.5) = -6 \cdot 16 \zeta(4) = -96 \zeta(4)
\]

Therefore, returning to \(I\):

\[
I = 8\psi^{(3)}(0.5) + 4\pi^4 (1+\sqrt{2}) + 384
= 8(-96\zeta(4)) + 4\pi^4(1+\sqrt{2}) + 384
= -768 \zeta(4) + 4\pi^4(1+\sqrt{2}) + 384
\]
Recall \(\zeta(4) = \frac{\pi^4}{90}\):

\[
= -768 \cdot \frac{\pi^4}{90} + 4\pi^4(1+\sqrt{2}) + 384
\]
\[
= \pi^4 \left(-\frac{768}{90} + 4(1+\sqrt{2})\right) + 384
\]
\[
-\frac{768}{90} = -\frac{256}{30} = -\frac{128}{15}
\]

Therefore,

\[
\boxed{I = \left[4(1+\sqrt{2}) - \frac{128}{15}\right]\pi^4 + 384}
\]

---

Let us compute the numerical value.

First, \(\pi^4\):
\[
\pi^4 = (\pi^2)^2 = (9.8696044011)^2 = 97.4090910340
\]

\(1+\sqrt{2} \approx 1 + 1.4142135624 = 2.4142135624\)

So,
\[
4(1+\sqrt{2}) = 4 \times 2.414213562373095 = 9.65685424949238
\]

Now,
\[
4(1+\sqrt{2}) - \frac{128}{15} = 9.65685424949238 - 8.53333333333333 = 1.12352091615905
\]

Now,
\[
1.12352091615905 \times 97.4090910340 = 109.448038299
\]

Add 384:
\[
I = 109.448038299 + 384 = 493.448038299
\]

Rounding to 10 decimals:
\[
I \approx 493.4480382990
\]

---

**Final Answer (as JSON):**
```json
{"answer": "\\left[4\\left(1 + \\sqrt{2}\\right) - \\frac{128}{15}\\right]\\pi^4 + 384", "numerical_answer": "493.4480382990"}
```