Let's compute the definite integral:
\[
I = \int_0^{\frac{\pi}{2}} x \ln(\sin x)\,dx
\]

**Step 1: Fourier Expansion of \(\ln(\sin x)\)**

Recall that:
\[
\ln(\sin x) = -\ln 2 - \sum_{k=1}^{\infty} \frac{\cos(2kx)}{k}
\]

So,
\[
I = \int_0^{\frac{\pi}{2}} x \left(-\ln 2 - \sum_{k=1}^{\infty} \frac{\cos(2kx)}{k}\right) dx
\]
\[
= -\ln 2 \int_0^{\frac{\pi}{2}} x dx - \sum_{k=1}^{\infty} \frac{1}{k} \int_0^{\frac{\pi}{2}} x \cos(2k x) dx
\]

The first integral:
\[
\int_0^{\frac{\pi}{2}} x dx = \left. \frac{x^2}{2} \right|_0^{\frac{\pi}{2}} = \frac{\pi^2}{8}
\]

So the first term is \(-\frac{\pi^2}{8} \ln 2\).

**Step 2: Compute \(\int_0^{\frac{\pi}{2}} x \cos(2k x) dx\)**

Use integration by parts:
Let \(u = x,\ dv = \cos(2k x)dx\), so \(du = dx\), \(v = \frac{\sin(2k x)}{2k}\).

\[
\int x \cos(2k x) dx = x \frac{\sin(2k x)}{2k} - \int \frac{\sin(2k x)}{2k} dx = x \frac{\sin(2k x)}{2k} + \frac{\cos(2k x)}{4k^2} + C
\]
(Because \(\int \sin(ax)\,dx = -\frac{1}{a}\cos(ax)\).)

Evaluate from \(0\) to \(\frac{\pi}{2}\):

First term: \(x \sin(2k x)/(2k)\) at \(x = \frac{\pi}{2}\): \(\frac{\pi}{2} \cdot \frac{\sin(k\pi)}{2k}\). At \(x = 0\): 0.

Second term: \(\frac{\cos(2k x)}{4k^2}\) at \(x = \frac{\pi}{2}\): \(\frac{\cos(k\pi)}{4k^2}\), at \(x=0\): \(\frac{1}{4k^2}\).

So,
\[
\int_0^{\frac{\pi}{2}} x \cos(2k x) dx = \frac{\pi}{2} \cdot \frac{\sin(k\pi)}{2k} + \frac{\cos(k\pi) - 1}{4k^2}
\]

But \(\sin(k\pi) = 0\), \(\cos(k\pi) = (-1)^k\).

So,
\[
\int_0^{\frac{\pi}{2}} x \cos(2k x) dx = \frac{(-1)^k - 1}{4k^2}
\]

**Step 3: Substitute Into the Series**

So,
\[
I = -\frac{\pi^2}{8} \ln 2 - \sum_{k=1}^{\infty} \frac{1}{k} \cdot \frac{(-1)^k - 1}{4k^2}
= -\frac{\pi^2}{8}\ln 2 - \frac{1}{4}\sum_{k=1}^{\infty} \frac{(-1)^k - 1}{k^3}
\]

Notice:
\[
(-1)^k - 1 = 
\begin{cases}
0 & \text{if } k \text{ even} \\
-2 & \text{if } k \text{ odd}
\end{cases}
\]

Therefore, the sum reduces to:
\[
\sum_{k=1}^\infty \frac{(-1)^k - 1}{k^3}
= -2 \sum_{n=0}^\infty \frac{1}{(2n+1)^3}
\]
That is, sum over odd \(k\).

So,
\[
I = -\frac{\pi^2}{8}\ln 2 + \frac{1}{2} \sum_{n=0}^\infty \frac{1}{(2n+1)^3}
\]

But the sum over all positive integers:
\[
\sum_{k=1}^\infty \frac{1}{k^s} = \zeta(s)
\]

Sum over odd integers:
\[
\sum_{n=0}^\infty \frac{1}{(2n+1)^s} = \sum_{k=1}^\infty \frac{1}{k^s} - \sum_{n=1}^\infty \frac{1}{(2n)^s}
= \zeta(s) - \frac{1}{2^s} \zeta(s)
= (1 - 2^{-s})\zeta(s)
\]

For \(s = 3\):
\[
\sum_{n=0}^\infty \frac{1}{(2n+1)^3} = (1 - 2^{-3})\zeta(3) = (1 - 1/8)\zeta(3) = \frac{7}{8}\zeta(3)
\]

Therefore,
\[
I = -\frac{\pi^2}{8}\ln 2 + \frac{1}{2} \cdot \frac{7}{8} \zeta(3) = -\frac{\pi^2}{8} \ln 2 + \frac{7}{16} \zeta(3)
\]

**Step 4: Numerical Approximation**

\[
\pi^2 \approx 9.8696044011
\]
\[
\ln 2 \approx 0.6931471806
\]
\[
\zeta(3) \approx 1.2020569032
\]

Compute:
\[
-\frac{\pi^2}{8} \ln 2 \approx -\frac{9.8696044011}{8} \cdot 0.6931471806 \approx -1.2337005501 \cdot 0.6931471806 \approx -0.8554905596
\]
\[
\frac{7}{16} \zeta(3) = 0.4375 \cdot 1.2020569032 \approx 0.5258978951
\]

Add:
\[
I \approx -0.8554905596 + 0.5258978951 = -0.3295926645
\]

**Final JSON Output (Only)**

```json
{"answer": "-\\frac{\\pi^2}{8}\\ln 2 + \\frac{7}{16}\\zeta(3)", "numerical_answer": "-0.3295926645"}
```