We start with the integral

  I = ∫[x=1/8]^(1/4) (ln(2x) · ln(4x) · ln(8x))⁄x dx.

Step 1. Substitute u = ln x so that du = dx/x. Then when:
  x = 1/8, u = ln(1/8) = –ln 8,
  x = 1/4, u = ln(1/4) = –ln 4.

Also note that
  ln(2x) = ln2 + u,
  ln(4x) = ln4 + u,
  ln(8x) = ln8 + u.

Thus the integral becomes

  I = ∫[u = -ln8]^( -ln4] (u + ln2)(u + ln4)(u + ln8) du.

Step 2. It is convenient to write ln4 and ln8 in terms of ln2:
  ln4 = 2 ln2 and ln8 = 3 ln2.

Then the product is

  (u + ln2)(u + 2ln2)(u + 3ln2).

First, multiply the first two factors:
  (u + ln2)(u + 2ln2) = u² + 3ln2·u + 2(ln2)².

Now, multiply by (u + 3ln2):
  (u² + 3ln2·u + 2(ln2)²)(u + 3ln2)
    = u³ + 3ln2·u² + 2(ln2)²·u + 3ln2·u² + 9(ln2)²·u + 6(ln2)³
    = u³ + 6ln2·u² + 11(ln2)²·u + 6(ln2)³.

Thus the integral becomes

  I = ∫[u = -ln8]^( -ln4] [ u³ + 6ln2·u² + 11(ln2)²·u + 6(ln2)³ ] du.

Step 3. Integrate term by term:
  ∫ u³ du = u⁴/4,
  ∫ u² du = u³/3,
  ∫ u du = u²/2,
  ∫ du = u.

Therefore, an antiderivative is

  F(u) = u⁴/4 + 6ln2·(u³/3) + 11(ln2)²·(u²/2) + 6(ln2)³·u
    = u⁴/4 + 2ln2·u³ + (11/2)(ln2)²·u² + 6(ln2)³·u.

Step 4. Evaluate F(u) from u = -ln8 to u = -ln4.
Recall:
  ln8 = 3 ln2 and ln4 = 2 ln2.

Thus, at u = -2 ln2:

  F(-2 ln2) = [(-2 ln2)⁴/4] + 2ln2·(-2 ln2)³ + (11/2)(ln2)²·(-2 ln2)² + 6(ln2)³·(-2 ln2).

Compute each term:
  Term1: (-2 ln2)⁴ = 16 (ln2)⁴ → 16/4 = 4 (ln2)⁴.
  Term2: (-2 ln2)³ = -8 (ln2)³ → 2ln2·(-8 (ln2)³) = -16 (ln2)⁴.
  Term3: (-2 ln2)² = 4 (ln2)² → (11/2)(ln2)²·4 (ln2)² = 22 (ln2)⁴.
  Term4: 6(ln2)³·(-2 ln2) = -12 (ln2)⁴.

Summing:
  4 (ln2)⁴ - 16 (ln2)⁴ + 22 (ln2)⁴ - 12 (ln2)⁴ = (-2)(ln2)⁴.

Next, at u = -3 ln2:

  F(-3 ln2) = [(-3 ln2)⁴/4] + 2ln2·(-3 ln2)³ + (11/2)(ln2)²·(-3 ln2)² + 6(ln2)³·(-3 ln2).

Compute:
  Term1: (-3 ln2)⁴ = 81 (ln2)⁴ → 81/4 (ln2)⁴.
  Term2: (-3 ln2)³ = -27 (ln2)³ → 2ln2·(-27 (ln2)³) = -54 (ln2)⁴.
  Term3: (-3 ln2)² = 9 (ln2)² → (11/2)(ln2)²·9 (ln2)² = 99/2 (ln2)⁴.
  Term4: 6(ln2)³·(-3 ln2) = -18 (ln2)⁴.

Express all with denominator 4:
  Term1: 81/4.
  Term2: -54 = -216/4.
  Term3: 99/2 = 198/4.
  Term4: -18 = -72/4.

Sum:
  (81 - 216 + 198 - 72)/4 = (-9)/4 (ln2)⁴.

Now, the definite integral is
  I = F(-2 ln2) - F(-3 ln2) = [ -2 (ln2)⁴ - ( -9/4 (ln2)⁴ ) ]
    = (-2 + 9/4)(ln2)⁴ = ( (-8/4 + 9/4) (ln2)⁴ ) = (1/4)(ln2)⁴.

Thus, the exact answer is

  I = (ln²2)⁴/4  or  I = (ln2)⁴/4.

Step 5. Numerical approximation.
We compute:
  ln2 ≈ 0.6931471806,
so
  (ln2)⁴ ≈ (0.6931471806)⁴ ≈ 0.2310490602,
and dividing by 4 gives
  I ≈ 0.2310490602/4 ≈ 0.0577622650.

Final Answer in JSON format:

{"answer": "\\frac{\\ln^4 2}{4}", "numerical_answer": "0.0577622650"}