We start with the integral

  I = ∫₀² x^(–1/2) · (2 – x)^(–1/2) cos(1.0·√(x(2–x))) dx.

Step 1. Substitute x = 1 – cosθ.
  • When x = 0, we have 0 = 1 – cosθ ⟹ cosθ = 1 ⟹ θ = 0.
  • When x = 2, we have 2 = 1 – cosθ ⟹ cosθ = –1 ⟹ θ = π.
  • Also, (2 – x) = 2 – (1 – cosθ) = 1 + cosθ.
  • The differential: dx = sinθ dθ.
  • Notice that the factors in the integrand become:
    x^(–1/2) = 1/√(1 – cosθ)  and  (2–x)^(–1/2) = 1/√(1+cosθ).
  • Their product is
    1/ [√(1 – cosθ)√(1 + cosθ)] = 1/√(1 – cos²θ) = 1/|sinθ|.
  Since θ ∈ [0, π], sinθ is nonnegative so |sinθ| = sinθ.

Step 2. Transform the integral.
  Substitute into I:
    I = ∫₀π [1/sinθ] · cos(√(x(2–x))) · (sinθ dθ).
  But note:
    x(2–x) = (1 – cosθ)(1 + cosθ) = 1 – cos²θ = sin²θ,
  so that √(x(2–x)) = sinθ.
  Thus,
    I = ∫₀π cos(sinθ) dθ.

Step 3. Recognize the standard Bessel function representation.
  There is a known integral representation of the Bessel function of order zero:
    J₀(z) = (1/π) ∫₀π cos(z sinθ) dθ.
  Taking z = 1, we have:
    ∫₀π cos(sinθ) dθ = π J₀(1).

Thus, the exact answer is

  I = π J₀(1).

Step 4. Numerical approximation.
  It is known that J₀(1) ≈ 0.7651976866, so
    I ≈ π × 0.7651976866 ≈ 2.4039394307.

The final answer in the required JSON format is:
{"answer": "\\pi J_{0}(1)", "numerical_answer": "2.4039394307"}