# Evaluating $\int_{0}^{1}{\frac{x^{3}+x+1}{3x^{2}-3x+4}}\:\mathrm{d}x$

I'll solve this definite integral step by step.

## Step 1: Polynomial Division
First, I'll perform polynomial division to simplify the integrand:

$$\frac{x^3+x+1}{3x^2-3x+4}$$

Let's divide $x^3+x+1$ by $3x^2-3x+4$:

$x^3 \div 3x^2 = \frac{x}{3}$

Multiply $\frac{x}{3} \cdot (3x^2-3x+4) = x^3-x^2+\frac{4x}{3}$

Subtract from the numerator:
$x^3+x+1 - (x^3-x^2+\frac{4x}{3}) = x^2+x-\frac{4x}{3}+1 = x^2+\frac{3x-4x}{3}+1 = x^2-\frac{x}{3}+1$

So we have:
$$\frac{x^3+x+1}{3x^2-3x+4} = \frac{x}{3} + \frac{x^2-\frac{x}{3}+1}{3x^2-3x+4}$$

## Step 2: Further Simplification
Let's simplify the remaining fraction. I'll multiply the numerator by $\frac{3}{3}$ to make it cleaner:

$$\frac{x^2-\frac{x}{3}+1}{3x^2-3x+4} = \frac{3x^2-x+3}{3(3x^2-3x+4)}$$

Now, let's try to express this in a form that's easier to integrate.

$$\frac{3x^2-x+3}{3(3x^2-3x+4)} = \frac{1}{3} \cdot \frac{3x^2-x+3}{3x^2-3x+4}$$

Let's examine $3x^2-x+3$ in relation to $3x^2-3x+4$:

$3x^2-3x+4 - (3x^2-x+3) = -3x+x+4-3 = -2x+1$

So:
$$\frac{3x^2-x+3}{3x^2-3x+4} = \frac{3x^2-3x+4-(-2x+1)}{3x^2-3x+4} = 1 - \frac{-2x+1}{3x^2-3x+4}$$

Thus:
$$\frac{x^3+x+1}{3x^2-3x+4} = \frac{x}{3} + \frac{1}{3} - \frac{-2x+1}{3(3x^2-3x+4)} = \frac{x+1}{3} + \frac{2x-1}{3(3x^2-3x+4)}$$

## Step 3: Partial Fractions for the Complex Term
For the fraction $\frac{2x-1}{3(3x^2-3x+4)}$, let's complete the square in the denominator:

$3x^2-3x+4 = 3(x^2-x+\frac{4}{3}) = 3(x^2-x+\frac{1}{4}+\frac{4}{3}-\frac{1}{4}) = 3((x-\frac{1}{2})^2+\frac{7}{12})$

Let $u = x-\frac{1}{2}$, then $3x^2-3x+4 = 3(u^2+\frac{7}{12})$

We have:
$$\frac{2x-1}{3(3x^2-3x+4)} = \frac{2x-1}{3 \cdot 3((x-\frac{1}{2})^2+\frac{7}{12})} = \frac{2x-1}{9((x-\frac{1}{2})^2+\frac{7}{12})}$$

When $x = u+\frac{1}{2}$, we get $2x-1 = 2(u+\frac{1}{2})-1 = 2u+1-1 = 2u$

So:
$$\frac{2x-1}{9((x-\frac{1}{2})^2+\frac{7}{12})} = \frac{2u}{9(u^2+\frac{7}{12})}$$

Now we can use the standard form:
$$\frac{du}{a^2+u^2} = \frac{1}{a} \arctan\left(\frac{u}{a}\right) + C$$

With $a^2 = \frac{7}{12}$, so $a = \sqrt{\frac{7}{12}} = \frac{\sqrt{7}}{\sqrt{12}} = \frac{\sqrt{7}}{2\sqrt{3}}$

## Step 4: Integration
Now, let's integrate each part:

$$\int \frac{x+1}{3} dx = \frac{x^2}{6} + \frac{x}{3} + C_1$$

For the complex term, we have:
$$\int \frac{2u}{9(u^2+\frac{7}{12})} du = \frac{2}{9} \int \frac{u}{u^2+\frac{7}{12}} du = \frac{2}{9} \cdot \frac{1}{2} \ln|u^2+\frac{7}{12}| + C_2 = \frac{1}{9} \ln|u^2+\frac{7}{12}| + C_2$$

Converting back to $x$, we get:
$$\frac{1}{9} \ln|(x-\frac{1}{2})^2+\frac{7}{12}| + C_2$$

So, the indefinite integral is:
$$\int \frac{x^3+x+1}{3x^2-3x+4} dx = \frac{x^2}{6} + \frac{x}{3} + \frac{1}{9} \ln|(x-\frac{1}{2})^2+\frac{7}{12}| + C$$

## Step 5: Evaluating the Definite Integral
Now we evaluate from $x=0$ to $x=1$:

At $x=1$:
$$\frac{1^2}{6} + \frac{1}{3} + \frac{1}{9} \ln|(1-\frac{1}{2})^2+\frac{7}{12}| = \frac{1}{6} + \frac{1}{3} + \frac{1}{9} \ln|\frac{1}{4}+\frac{7}{12}| = \frac{1}{6} + \frac{1}{3} + \frac{1}{9} \ln|\frac{3+7}{12}| = \frac{1}{6} + \frac{1}{3} + \frac{1}{9} \ln|\frac{10}{12}| = \frac{1}{6} + \frac{1}{3} + \frac{1}{9} \ln|\frac{5}{6}|$$

At $x=0$:
$$\frac{0^2}{6} + \frac{0}{3} + \frac{1}{9} \ln|(0-\frac{1}{2})^2+\frac{7}{12}| = 0 + 0 + \frac{1}{9} \ln|\frac{1}{4}+\frac{7}{12}| = \frac{1}{9} \ln|\frac{3+7}{12}| = \frac{1}{9} \ln|\frac{10}{12}| = \frac{1}{9} \ln|\frac{5}{6}|$$

The definite integral is:
$$\left(\frac{1}{6} + \frac{1}{3} + \frac{1}{9} \ln|\frac{5}{6}|\right) - \left(\frac{1}{9} \ln|\frac{5}{6}|\right) = \frac{1}{6} + \frac{1}{3} = \frac{1}{6} + \frac{2}{6} = \frac{3}{6} = \frac{1}{2}$$

## Step 6: Numerical Approximation
The exact value is $\frac{1}{2}$, which as a decimal is $0.5000000000$ (to 10 decimal places).

So our final answer is $\frac{1}{2}$.

{"answer": "\\frac{1}{2}", "numerical_answer": "0.5000000000"}