<think>
Okay, let's see. I need to compute the definite integral from 420 to 1672 of [sqrt(ln(2023 - x)) divided by (sqrt(ln(2023 - x)) + sqrt(ln(x - 69)))] dx. Hmm, that looks a bit complicated, but maybe there's a substitution or symmetry I can use here.

First, let me check the limits of integration. The lower limit is 420, and the upper limit is 1672. The integrand involves ln(2023 - x) and ln(x - 69). Let me see what happens if I substitute x with something that might simplify the expression. Often in integrals with symmetric-looking denominators, substituting x = a + b - t can help. Let's try that.

Let me set t = 2023 - x + 69. Wait, maybe not. Let me think. The arguments inside the logarithms are 2023 - x and x - 69. Let me check the sum of these two: (2023 - x) + (x - 69) = 2023 - 69 = 1954. So, 2023 - x and x - 69 add up to 1954. That's a constant. That suggests that if I substitute x such that t = 2023 - x + (x - 69) = 1954, but that's just a constant. Maybe a substitution where t = 2023 - (x - 69) = 2023 - x + 69? Wait, maybe not. Let me think again.

Alternatively, if I let t = 2023 - x + 69, but that's 2092 - x. Hmm, maybe not. Wait, perhaps a substitution that swaps 2023 - x and x - 69. Let me try substituting t = 2023 - (x - 69) + 69? Wait, that's confusing. Let me try a substitution.

Let me set t = 2023 - x + (x - 69) = 1954, but that's a constant. Not helpful. Wait, maybe if I let t = 2023 - x, then x = 2023 - t. Let's try that substitution. Then when x = 420, t = 2023 - 420 = 1603. When x = 1672, t = 2023 - 1672 = 351. So the limits would be from t = 1603 to t = 351. But integrating from 1603 to 351 would be the same as integrating from 351 to 1603 with a negative sign. Let's see:

dx = -dt, so the integral becomes ∫ from t=1603 to t=351 of [sqrt(ln(t)) / (sqrt(ln(t)) + sqrt(ln(2023 - (2023 - t) - 69)))] (-dt). Wait, let me check the substitution again. If x = 2023 - t, then x - 69 = 2023 - t - 69 = 1954 - t. So the denominator becomes sqrt(ln(t)) + sqrt(ln(1954 - t)). The numerator is sqrt(ln(t)). So the integrand becomes sqrt(ln(t)) / [sqrt(ln(t)) + sqrt(ln(1954 - t))] * (-dt). But since we're integrating from 1603 to 351, the negative sign reverses the limits to 351 to 1603, so the integral becomes ∫ from 351 to 1603 of sqrt(ln(t)) / [sqrt(ln(t)) + sqrt(ln(1954 - t))] dt.

But the original integral was from 420 to 1672. Wait, maybe I need to check the substitution again. Let me write it step by step.

Original integral: Let x go from 420 to 1672. Let t = 2023 - x. Then when x = 420, t = 2023 - 420 = 1603. When x = 1672, t = 2023 - 1672 = 351. So the substitution gives us:

∫_{x=420}^{1672} [sqrt(ln(2023 - x)) / (sqrt(ln(2023 - x)) + sqrt(ln(x - 69)))] dx

= ∫_{t=1603}^{351} [sqrt(ln(t)) / (sqrt(ln(t)) + sqrt(ln(2023 - (2023 - t) - 69)))] (-dt)

Wait, x - 69 = (2023 - t) - 69 = 2023 - 69 - t = 1954 - t. So ln(x - 69) = ln(1954 - t). Therefore, the integrand becomes sqrt(ln(t)) / [sqrt(ln(t)) + sqrt(ln(1954 - t))] * (-dt). The limits are from t=1603 to t=351, so reversing the limits removes the negative sign:

= ∫_{t=351}^{1603} [sqrt(ln(t)) / (sqrt(ln(t)) + sqrt(ln(1954 - t)))] dt

But the original integral is in terms of x, and after substitution, we have an integral in terms of t. Let's call the original integral I. Then:

I = ∫_{420}^{1672} [sqrt(ln(2023 - x)) / (sqrt(ln(2023 - x)) + sqrt(ln(x - 69)))] dx

After substitution, I = ∫_{351}^{1603} [sqrt(ln(t)) / (sqrt(ln(t)) + sqrt(ln(1954 - t)))] dt

Now, notice that the original integral's limits are from 420 to 1672. Let me check what 420 and 1672 are in terms of the substitution. Wait, 420 is the lower limit, and 1672 is the upper limit. But after substitution, the limits become 1603 (when x=420) to 351 (when x=1672). Then reversing gives 351 to 1603.

But perhaps there's a symmetry here. Let me consider adding the original integral I and the substituted integral. Let me write:

I = ∫_{420}^{1672} [sqrt(ln(2023 - x)) / (sqrt(ln(2023 - x)) + sqrt(ln(x - 69)))] dx

After substitution, I = ∫_{351}^{1603} [sqrt(ln(t)) / (sqrt(ln(t)) + sqrt(ln(1954 - t)))] dt

But if I rename the variable t back to x in the substituted integral, then:

I = ∫_{351}^{1603} [sqrt(ln(x)) / (sqrt(ln(x)) + sqrt(ln(1954 - x)))] dx

Now, if I add the original integral and this substituted integral, but wait, the original integral is from 420 to 1672, and this substituted integral is from 351 to 1603. Hmm, maybe not directly additive. Wait, perhaps there's another substitution that can relate these.

Alternatively, let's consider another substitution in the original integral. Let me set u = 2023 - x + (x - 69) = 1954, but that's a constant. Not helpful. Wait, perhaps another substitution: Let u = (x - 69) + (2023 - x) = 1954, which is the same as before. Hmm.

Wait, maybe if I make a substitution in the original integral where u = 1954 - t, but not sure. Let me think again.

Alternatively, let's consider that the integrand has the form f(x) = sqrt(ln(a - x)) / [sqrt(ln(a - x)) + sqrt(ln(x - b))], where a = 2023 and b = 69. Then, perhaps using the substitution u = a + b - x, which would be 2023 + 69 - x = 2092 - x. Let's try that substitution.

Let u = 2092 - x. Then when x = 420, u = 2092 - 420 = 1672. When x = 1672, u = 2092 - 1672 = 420. So the limits would reverse from 1672 to 420. Then dx = -du. Let's compute the integrand in terms of u.

Original integrand: sqrt(ln(2023 - x)) / [sqrt(ln(2023 - x)) + sqrt(ln(x - 69))]

With u = 2092 - x, then 2023 - x = 2023 - (2092 - u) = 2023 - 2092 + u = u - 69. Similarly, x - 69 = (2092 - u) - 69 = 2023 - u. So the integrand becomes sqrt(ln(u - 69)) / [sqrt(ln(u - 69)) + sqrt(ln(2023 - u))].

Therefore, the integral becomes:

∫_{x=420}^{1672} [sqrt(ln(2023 - x)) / (sqrt(ln(2023 - x)) + sqrt(ln(x - 69)))] dx

= ∫_{u=1672}^{420} [sqrt(ln(u - 69)) / (sqrt(ln(u - 69)) + sqrt(ln(2023 - u)))] (-du)

= ∫_{420}^{1672} [sqrt(ln(u - 69)) / (sqrt(ln(u - 69)) + sqrt(ln(2023 - u)))] du

But since u is a dummy variable, we can write this as:

I = ∫_{420}^{1672} [sqrt(ln(x - 69)) / (sqrt(ln(x - 69)) + sqrt(ln(2023 - x)))] dx

So now, the original integral I is equal to the integral of the other term in the denominator. Let me denote the original integral as I. Then, from the above substitution, we have:

I = ∫_{420}^{1672} [sqrt(ln(2023 - x)) / (sqrt(ln(2023 - x)) + sqrt(ln(x - 69)))] dx

And also:

I = ∫_{420}^{1672} [sqrt(ln(x - 69)) / (sqrt(ln(x - 69)) + sqrt(ln(2023 - x)))] dx

If I add these two expressions for I, I get:

I + I = ∫_{420}^{1672} [sqrt(ln(2023 - x)) + sqrt(ln(x - 69))] / [sqrt(ln(2023 - x)) + sqrt(ln(x - 69))] dx

The numerator and denominator are the same, so this simplifies to:

2I = ∫_{420}^{1672} 1 dx = (1672 - 420) = 1252

Therefore, 2I = 1252, so I = 1252 / 2 = 626.

So the exact value of the integral is 626. That's a neat result from exploiting the symmetry in the integrand. 

Now, the numerical approximation. Since the exact answer is 626, the numerical approximation is just 626.0000000000 when rounded to 10 decimal places. But let me confirm that there's no calculation errors here. The key step was recognizing the substitution u = 2023 + 69 - x = 2092 - x, which swaps the terms in the numerator and denominator. Adding the two integrals gives the integral of 1 over the interval, which is the length of the interval. Therefore, the answer is indeed (1672 - 420)/2 = 1252/2 = 626. 

So the exact answer is 626, and numerically it's 626.0000000000.
</think>

{"answer": "626", "numerical_answer": "626.0000000000"}