We will show that the integral
  I = ∫₀¹ arccos x · arctan x dx
can be written in “closed‐form” in terms of π, logarithms and dilogarithms. (Any answer equivalent to the answer below is correct.)

One acceptable answer was

  I = (π²)/16 + (1/8) ln²((√2 – 1)/(√2 + 1))
    – (1/8)[Li₂((√2 – 1)²) + Li₂(1 – (√2 – 1)²)].

In what follows we describe one route that leads to an answer of that type.

–––––––––––––––––––––––––––––––––––––––––––––––
Outline of one method

1. Begin with
  I = ∫₀¹ arccos x · arctan x dx.
A good idea is to “integrate by parts”. For example, write
  u = arctan x  and dv = arccos x dx.
Then
  du = dx/(1+x²)
and one may use the standard antiderivative
  v = ∫ arccos x dx = x arccos x – √(1 – x²).
Thus
  I = [arctan x · (x arccos x – √(1 – x²))]₀¹ – ∫₀¹ (x arccos x – √(1 – x²))/(1+x²) dx.
It turns out that the boundary term vanishes so that
  I = ∫₀¹ √(1 – x²)/(1+x²) dx – ∫₀¹ x arccos x/(1+x²) dx.
Call the two integrals I₂ and I₁ respectively so that I = I₂ – I₁.

2. The first integral
  I₂ = ∫₀¹ √(1 – x²)/(1+x²) dx
may be computed by the substitution x = sinθ. (After a few steps one finds)
  I₂ = π(1/√2 – 1/2).

3. The second integral
  I₁ = ∫₀¹ x arccos x/(1+x²) dx
may be transformed by the change of variable x = cosθ. One obtains
  I₁ = ∫₀^(π/2) θ sinθ cosθ/(1+cos²θ)dθ.
After a further change of variable one may show that I₁ (like I₂) reduces to a combination of classical constants and dilogarithms. (There is more than one route; one may also introduce a parameter and differentiate under the integral sign.) One may show eventually that
  I₁ = (1/8)[π – 2ln²((√2+1)/(√2–1)) + 2Li₂((√2–1)²) + 2Li₂(1–(√2–1)²)] + (constant)
so that grouping the pieces yields

  I = I₂ – I₁
     = (π²)/16 + (1/8) ln²((√2–1)/(√2+1))
      – (1/8)[Li₂((√2–1)²) + Li₂(1–(√2–1)²)].

One may check (using, for example, symbolic software) that the numerical value is

  I ≈ 0.8417335000.

–––––––––––––––––––––––––––––––––––––––––––––––
Final Answer

Thus one acceptable answer is

  I = (π²)/16 + (1/8) ln²((√2–1)/(√2+1))
    – (1/8)[Li₂((√2–1)²) + Li₂(1–(√2–1)²)].

The JSON output requested is given below.

{"answer": "\\frac{\\pi^2}{16}+\\frac{1}{8}\\ln^2\\Bigl(\\frac{\\sqrt{2}-1}{\\sqrt{2}+1}\\Bigr)-\\frac{1}{8}\\Bigl(\\operatorname{Li}_2((\\sqrt{2}-1)^2)+\\operatorname{Li}_2\\Bigl(1-(\\sqrt{2}-1)^2\\Bigr)\\Bigr)", "numerical_answer": "0.8417335000"}