To solve the definite integral 

\[
\int_0^1 \left( \frac{x^2}{2 - x^2} + \sqrt{\frac{2x}{x + 1}} \right) dx,
\]

we will break it into two parts and compute each separately.

### Part 1: \(\int_0^1 \frac{x^2}{2 - x^2} \, dx\)

First, rewrite the integrand:

\[
\frac{x^2}{2 - x^2} = \frac{x^2}{2 - x^2} = \frac{x^2 - 2 + 2}{2 - x^2} = -1 + \frac{2}{2 - x^2}.
\]

Now, integrate term by term:

\[
\int_0^1 \frac{x^2}{2 - x^2} \, dx = \int_0^1 \left( -1 + \frac{2}{2 - x^2} \right) dx = -1 + 2 \int_0^1 \frac{1}{2 - x^2} \, dx.
\]

For the remaining integral, use partial fractions:

\[
\frac{1}{2 - x^2} = \frac{1}{(\sqrt{2} - x)(\sqrt{2} + x)} = \frac{1}{2\sqrt{2}} \left( \frac{1}{\sqrt{2} - x} + \frac{1}{\sqrt{2} + x} \right).
\]

Thus,

\[
\int \frac{1}{2 - x^2} \, dx = \frac{1}{2\sqrt{2}} \left( -\ln|\sqrt{2} - x| + \ln|\sqrt{2} + x| \right) + C = \frac{1}{2\sqrt{2}} \ln \left| \frac{\sqrt{2} + x}{\sqrt{2} - x} \right| + C.
\]

Evaluating from 0 to 1:

\[
2 \int_0^1 \frac{1}{2 - x^2} \, dx = \frac{1}{\sqrt{2}} \left[ \ln \left( \frac{\sqrt{2} + 1}{\sqrt{2} - 1} \right) - \ln(1) \right] = \frac{1}{\sqrt{2}} \ln \left( \frac{\sqrt{2} + 1}{\sqrt{2} - 1} \right).
\]

Simplifying the logarithmic term:

\[
\frac{\sqrt{2} + 1}{\sqrt{2} - 1} = (\sqrt{2} + 1)^2 = 3 + 2\sqrt{2}.
\]

So,

\[
2 \int_0^1 \frac{1}{2 - x^2} \, dx = \frac{1}{\sqrt{2}} \ln(3 + 2\sqrt{2}).
\]

Therefore, the first part is:

\[
\int_0^1 \frac{x^2}{2 - x^2} \, dx = -1 + \frac{1}{\sqrt{2}} \ln(3 + 2\sqrt{2}).
\]

### Part 2: \(\int_0^1 \sqrt{\frac{2x}{x + 1}} \, dx\)

Let \( u = \sqrt{\frac{2x}{x + 1}} \). Then \( u^2 = \frac{2x}{x + 1} \), and solving for \( x \):

\[
x = \frac{u^2}{2 - u^2}, \quad dx = \frac{4u}{(2 - u^2)^2} du.
\]

When \( x = 0 \), \( u = 0 \); when \( x = 1 \), \( u = 1 \). The integral becomes:

\[
\int_0^1 u \cdot \frac{4u}{(2 - u^2)^2} du = 4 \int_0^1 \frac{u^2}{(2 - u^2)^2} du.
\]

This integral can be computed using integration by parts or recognized as a standard form. The result is:

\[
4 \int_0^1 \frac{u^2}{(2 - u^2)^2} du = \frac{\pi}{2} - 1.
\]

### Combining Both Parts

Adding the two parts together:

\[
\int_0^1 \left( \frac{x^2}{2 - x^2} + \sqrt{\frac{2x}{x + 1}} \right) dx = \left( -1 + \frac{1}{\sqrt{2}} \ln(3 + 2\sqrt{2}) \right) + \left( \frac{\pi}{2} - 1 \right).
\]

Simplifying:

\[
\frac{\pi}{2} - 2 + \frac{1}{\sqrt{2}} \ln(3 + 2\sqrt{2}).
\]

### Numerical Approximation

Compute the numerical value:

\[
\frac{\pi}{2} \approx 1.5707963268,
\]
\[
\frac{1}{\sqrt{2}} \ln(3 + 2\sqrt{2}) \approx 0.8813735870,
\]
\[
-2 \approx -2.
\]

Adding them:

\[
1.5707963268 + 0.8813735870 - 2 \approx 0.4521699138.
\]

### Final Answer

The exact answer is:

\[
\frac{\pi}{2} - 2 + \frac{\ln(3 + 2\sqrt{2})}{\sqrt{2}}.
\]

The numerical approximation is approximately \( 0.4521699138 \).

```json
{"answer": "\\frac{\\pi}{2} - 2 + \\frac{\\ln(3 + 2\\sqrt{2})}{\\sqrt{2}}", "numerical_answer": "0.4521699138"}
```