We start with 
  I = ∫₀² [1/(x(2–x))] arctan(√(x(2–x))) dx.

Step 1. Change of variable

Let
  x = 1 – cos t.
Then
  2 – x = 1 + cos t  and  dx = sin t dt.
Also, note that
  x(2 – x) = (1 – cos t)(1 + cos t) = 1 – cos²t = sin²t,
so that
  √(x(2 – x)) = sin t  (for t between 0 and π).

We also have
  x⁻¹(2–x)⁻¹ = 1/[(1–cos t)(1+cos t)] = 1/sin²t.

Now, we must adjust the limits. When

  x = 0 → 0 = 1 – cos t → cos t = 1 → t = 0,
  x = 2 → 2 = 1 – cos t → cos t = –1 → t = π.

Thus, the integral becomes

  I = ∫₀ᴨ [1/sin²t] · arctan(sin t) · (sin t dt)
     = ∫₀ᴨ [arctan(sin t)/ sin t] dt.

Step 2. Exploiting symmetry

Notice that sin t is symmetric about t = π/2. So we can write

  I = 2∫₀^(π/2) [arctan(sin t)/ sin t] dt.
Let us denote
  J = ∫₀^(π/2) [arctan(sin t)/ sin t] dt,
so that I = 2J.

Step 3. Representing arctan and Interchanging Integration

We use the representation
  arctan z = ∫₀¹ [z/(1 + u²z²)] du  (for z ≥ 0).
Setting z = sin t gives
  arctan(sin t) = ∫₀¹ [sin t/(1 + u² sin²t)] du.

Thus,
  J = ∫₀^(π/2) [1/sin t] · {∫₀¹ [sin t/(1+u² sin²t)] du} dt.
The sin t cancels:
  J = ∫₀^(π/2) ∫₀¹ 1/(1+u² sin²t) du dt.
By Fubini’s theorem (since the integrals converge) we switch the order:

  J = ∫₀¹ du ∫₀^(π/2) [dt/(1+u² sin²t)].

Step 4. Evaluating the t‐integral

A standard formula tells us that
  ∫₀^(π/2) [dt/(1+m sin²t)] = (π/2)/√(1+m),
with m = u². Hence,

  ∫₀^(π/2) [dt/(1+u² sin²t)] = (π/2)/√(1+u²).

Thus,
  J = ∫₀¹ (π/2)/√(1+u²) du = (π/2) ∫₀¹ du/√(1+u²).

Step 5. Evaluating the u‐integral

We recognize the antiderivative:
  ∫ du/√(1+u²) = asinh(u) = ln(u + √(1+u²)).
Evaluating from 0 to 1 we obtain:
  ∫₀¹ du/√(1+u²) = asinh(1) – asinh(0) = asinh(1) = ln(1+√2).

Thus,
  J = (π/2) ln(1+√2)
and therefore
  I = 2J = π ln(1+√2).

Step 6. Numerical approximation

Using
  √2 ≈ 1.4142135624  and  ln(1+√2) = ln(2.4142135624) ≈ 0.881373,
we have
  I ≈ 3.1415926536 × 0.881373 ≈ 2.7690700000.

Final Answer in JSON:
{"answer": "\\pi \\ln\\left(1+\\sqrt{2}\\right)", "numerical_answer": "2.7690700000"}