

To solve the definite integral \(\int_{0}^{1} \frac{x^3 + x + 1}{3x^2 - 3x + 4} \, dx\), we follow these steps:

### Step 1: Polynomial Long Division
The integrand is a rational function where the numerator (degree 3) has a higher degree than the denominator (degree 2). We perform polynomial long division to simplify the integrand:

Dividing \(x^3 + x + 1\) by \(3x^2 - 3x + 4\):
- The leading term of the quotient is \(\frac{x}{3}\). Multiplying the denominator by \(\frac{x}{3}\) gives \(x^3 - x^2 + \frac{4x}{3}\).
- Subtracting this from the numerator leaves a remainder of \(x^2 - \frac{x}{3} + 1\).
- The next term in the quotient is \(\frac{1}{3}\). Multiplying the denominator by \(\frac{1}{3}\) gives \(x^2 - x + \frac{4}{3}\).
- Subtracting this from the remainder leaves a final remainder of \(\frac{2x}{3} - \frac{1}{3}\).

Thus, the integrand simplifies to:
\[
\frac{x^3 + x + 1}{3x^2 - 3x + 4} = \frac{x + 1}{3} + \frac{2x - 1}{3(3x^2 - 3x + 4)}.
\]

### Step 2: Split the Integral
We split the integral into two parts:
\[
\int_{0}^{1} \frac{x^3 + x + 1}{3x^2 - 3x + 4} \, dx = \int_{0}^{1} \frac{x + 1}{3} \, dx + \int_{0}^{1} \frac{2x - 1}{3(3x^2 - 3x + 4)} \, dx.
\]

### Step 3: Evaluate the First Integral
The first integral is straightforward:
\[
\int_{0}^{1} \frac{x + 1}{3} \, dx = \frac{1}{3} \int_{0}^{1} (x + 1) \, dx = \frac{1}{3} \left[ \frac{x^2}{2} + x \right]_{0}^{1} = \frac{1}{3} \left( \frac{1}{2} + 1 \right) = \frac{1}{2}.
\]

### Step 4: Evaluate the Second Integral
For the second integral, notice that the numerator \(2x - 1\) is proportional to the derivative of the denominator \(3x^2 - 3x + 4\) (since \(\frac{d}{dx}(3x^2 - 3x + 4) = 6x - 3 = 3(2x - 1)\)). Let \(u = 3x^2 - 3x + 4\), so \(du = 3(2x - 1) \, dx\) or \((2x - 1) \, dx = \frac{du}{3}\). The integral becomes:
\[
\int_{0}^{1} \frac{2x - 1}{3(3x^2 - 3x + 4)} \, dx = \frac{1}{3} \int_{u(0)}^{u(1)} \frac{1}{3u} \, du = \frac{1}{9} \left[ \ln|u| \right]_{4}^{4} = \frac{1}{9} (\ln 4 - \ln 4) = 0.
\]

### Step 5: Combine Results
Adding the results of the two integrals gives:
\[
\int_{0}^{1} \frac{x^3 + x + 1}{3x^2 - 3x + 4} \, dx = \frac{1}{2} + 0 = \frac{1}{2}.
\]

### Numerical Approximation
The exact value is \(\frac{1}{2}\), so the numerical approximation (rounded to 10 decimal places) is \(0.5\).

{"answer": "\\frac{1}{2}", "numerical_answer": "0.5000000000"}