Let's solve the integral:
\[
I = \int_{0}^{1} \frac{x^3 + x + 1}{3x^2 - 3x + 4} \, dx
\]

**Step 1: Analytically Solve**

First, let's try to split the numerator to aid in integration.

Notice that the denominator is quadratic in \(x\):
\[
3x^2 - 3x + 4
\]

Let’s attempt to write the numerator as:
\[
x^3 + x + 1 = A(3x^2 - 3x + 4) + Bx + C
\]
But this gives 3rd order, so instead, perform polynomial long division:

### Polynomial Long Division

Divide \(x^3 + x + 1\) by \(3x^2 - 3x + 4\):

- \(x^3 / 3x^2 = (1/3)x\)
- Multiply back: \((1/3)x \cdot (3x^2 - 3x + 4) = x^3 - x^2 + (4/3)x\)
- Subtract: \(x^3 + x + 1 - (x^3 - x^2 + (4/3)x) = x^2 + x + 1 - (4/3)x = x^2 + x - (4/3)x + 1 = x^2 + (x - (4/3)x) + 1 = x^2 - (1/3)x + 1\)

Now, divide \(x^2 - (1/3)x + 1\) by \(3x^2 - 3x + 4\):
- Highest degree is lower, so this is the remainder.

So,
\[
\frac{x^3 + x + 1}{3x^2 - 3x + 4} = \frac{1}{3}x + \frac{x^2 - \frac{1}{3}x + 1}{3x^2 - 3x + 4}
\]

Let’s focus on integrating both terms:
\[
I = \int_{0}^{1} \left[ \frac{1}{3}x + \frac{x^2 - \frac{1}{3}x + 1}{3x^2 - 3x + 4} \right] dx
\]

#### Integrate the first term:
\[
\int_{0}^{1} \frac{1}{3}x \, dx = \frac{1}{3}\left[\frac{1}{2}x^2 \right]_{0}^{1} = \frac{1}{3} \cdot \frac{1}{2} = \frac{1}{6}
\]

#### Now, for the second term:
We seek to express \(x^2 - \frac{1}{3}x + 1\) in terms of the derivative of denominator, plus a constant.

Let’s compute the derivative of denominator:
\[
\frac{d}{dx}\left(3x^2 - 3x + 4\right) = 6x - 3
\]
Let’s write:
\[
x^2 - \frac{1}{3} x + 1 = A(6x - 3) + B
\]
Wait, let's instead express \(x^2 - \frac{1}{3}x + 1 = A(3x^2 - 3x + 4)' + B\)
That is,
\[
x^2 - \frac{1}{3}x + 1 = A(6x - 3) + B
\]
Equate coefficients:
- \(x^2\): Only appears on LHS, so must come from something else – maybe try substitution instead.

Alternatively, write:
\[
x^2 - \frac{1}{3}x + 1 = A(3x^2 - 3x + 4) + B(6x - 3) + C
\]
Expand:
\[
A(3x^2 - 3x + 4) = 3A x^2 - 3A x + 4A \\
B(6x - 3) = 6B x - 3B \\
\]
So,
\[
x^2 - \frac{1}{3}x + 1 = 3A x^2 - 3A x + 4A + 6B x - 3B + C
\]
Collect like terms:
- \(x^2:\) \(3A\)
- \(x:\) \(-3A + 6B\)
- constant: \(4A - 3B + C\)

Equate:
1. \(x^2\): \(3A = 1 \implies A = \frac{1}{3}\)
2. \(x:\) \(-3A + 6B = -\frac{1}{3}\)
   Plug in \(A = 1/3\):
   \(-3 \cdot (1/3) + 6B = -1 + 6B = -\frac{1}{3}\)
   \(6B = -\frac{1}{3} + 1 = \frac{2}{3}\)
   \(B = \frac{1}{9}\)
3. Constants:\(4A - 3B + C = 1\)
   Plug in above:
   \(4 \cdot (1/3) - 3 \cdot (1/9) + C = \frac{4}{3} - \frac{1}{3} + C = 1 + C\)
   Therefore, \(1 + C = 1 \implies C = 0\)

So,
\[
x^2 - \frac{1}{3}x + 1 = \frac{1}{3}(3x^2 - 3x + 4) + \frac{1}{9}(6x - 3)
\]

Thus,
\[
\frac{x^2 - \frac{1}{3}x + 1}{3x^2 - 3x + 4} = \frac{1}{3} + \frac{1}{9} \cdot \frac{6x - 3}{3x^2 - 3x + 4}
\]

Substitute back:
\[
I = \frac{1}{6} + \int_0^1 \left(\frac{1}{3} + \frac{1}{3} + \frac{1}{9} \frac{6x-3}{3x^2 - 3x + 4}\right) dx
\]
\[
= \frac{1}{6} + \frac{2}{3} \int_0^1 dx + \frac{1}{9} \int_0^1 \frac{6x-3}{3x^2 - 3x + 4} dx
\]
\[
\int_0^1 dx = 1
\]
So,
\[
I = \frac{1}{6} + \frac{2}{3} + \frac{1}{9} \int_0^1 \frac{6x-3}{3x^2 - 3x + 4} dx
\]
\[
= \frac{5}{6} + \frac{1}{9} \int_0^1 \frac{6x-3}{3x^2 - 3x + 4} dx
\]

Let’s compute \(J = \int_0^1 \frac{6x-3}{3x^2 - 3x + 4} dx\)

Notice that \(6x-3\) is exactly the derivative of \(3x^2 - 3x + 4\):

\[
d/dx (3x^2 - 3x + 4) = 6x - 3
\]

Thus,
\[
\int \frac{6x - 3}{3x^2 - 3x + 4} dx = \ln|3x^2 - 3x + 4| + C
\]
So
\[
J = [\ln(3x^2 - 3x + 4)]_0^1
\]
At \(x = 1\):
\[
3(1)^2 - 3(1) + 4 = 3 - 3 + 4 = 4
\]
At \(x = 0\):
\[
3(0)^2 - 3(0) + 4 = 4
\]
Hence,
\[
J = \ln 4 - \ln 4 = 0
\]

Thus,
\[
I = \frac{5}{6} + \frac{1}{9} \cdot 0 = \frac{5}{6}
\]

---

**Step 3: Numerical Approximation**

\[
\frac{5}{6} = 0.8333333333
\]

---

**Final Output:**

```json
{"answer": "\\frac{5}{6}", "numerical_answer": "0.8333333333"}
```