Let's solve the integral:
\[
\int_1^2\frac{9x+4}{x^5+3x^2+x}\ dx
\]

**Step 1: Factor the Denominator**

The denominator:
\[
x^5 + 3x^2 + x = x(x^4 + 3x + 1)
\]
But \(x^4 + 3x + 1\) doesn't factor nicely; let's see if we can proceed with partial fractions.

**Step 2: Partial Fraction Decomposition**

Write:
\[
\frac{9x+4}{x(x^4 + 3x + 1)}
= \frac{A}{x} + \frac{Bx^3 + Cx^2 + Dx + E}{x^4 + 3x + 1}
\]

Multiply both sides by the denominator:
\[
9x + 4 = A(x^4 + 3x + 1) + (Bx^3 + Cx^2 + Dx + E)x
\]
\[
= A x^4 + 3A x + A + B x^4 + C x^3 + D x^2 + E x
\]

Now group like powers of \(x\):

- \(x^4:\) \(A + B\)
- \(x^3:\) \(C\)
- \(x^2:\) \(D\)
- \(x^1:\) \(3A + E\)
- constant: \(A\)

Set equal to original numerator \(9x + 4\):

Comparing coefficients:

- For \(x^4:\) \(A + B = 0\)
- For \(x^3:\) \(C = 0\)
- For \(x^2:\) \(D = 0\)
- For \(x^1:\) \(3A + E = 9\)
- For constant: \(A = 4\)

Now solve:

- \(A = 4\)
- \(C = 0\)
- \(D = 0\)
- \(A + B = 0 \implies B = -A = -4\)
- \(3A + E = 9 \implies 3\times 4 + E = 9 \implies E = 9 - 12 = -3\)

Thus:

\[
A = 4,\quad B = -4,\quad C = 0,\quad D = 0,\quad E = -3
\]

That is,
\[
\frac{9x+4}{x(x^4 + 3x + 1)} = \frac{4}{x} + \frac{-4x^3 - 3}{x^4 + 3x + 1}
\]

**Step 3: Write the Integral**

\[
\int_1^2\frac{9x+4}{x^5+3x^2+x}\ dx =
\int_1^2 \left( \frac{4}{x} - \frac{4x^3 + 3}{x^4 + 3x + 1} \right) dx
\]

Break up:
\[
= 4\int_1^2 \frac{dx}{x} - \int_1^2 \frac{4x^3 + 3}{x^4 + 3x + 1}\ dx
\]

Let's consider the second part:
\[
\int \frac{4x^3 + 3}{x^4 + 3x + 1} dx
\]

Letâ€™s differentiate denominator:
\[
\frac{d}{dx}(x^4 + 3x + 1) = 4x^3 + 3
\]
Exactly matches the numerator!

So,
\[
\int \frac{4x^3 + 3}{x^4 + 3x + 1}\ dx = \ln|x^4+3x+1| + C
\]

**Therefore:**

\[
\int_1^2\frac{9x+4}{x^5+3x^2+x}\ dx
= 4 \int_1^2 \frac{dx}{x} - \int_1^2 \frac{4x^3+3}{x^4+3x+1}dx
\]
\[
= 4 \left[ \ln x \right]_1^2 - \left[ \ln(x^4+3x+1) \right]_1^2
\]
\[
= 4(\ln 2 - \ln 1) - [\ln(x^4 + 3x + 1)\big|_{x=1}^{x=2}]
\]
\[
= 4 \ln 2 - [\ln(2^4+3\times2+1) - \ln(1^4 + 3\times1 + 1)]
\]
\[
= 4 \ln 2 - [\ln(16+6+1) - \ln(1+3+1)]
\]
\[
= 4 \ln 2 - [\ln(23) - \ln(5)]
\]
\[
= 4 \ln 2 - \ln 23 + \ln 5
\]
\[
= 4 \ln 2 + \ln 5 - \ln 23
\]

Combine logs:
\[
4 \ln 2 + \ln 5 - \ln 23 = \ln(2^4) + \ln 5 - \ln 23 = \ln(16) + \ln 5 - \ln 23 = \ln(16 \cdot 5) - \ln(23) = \ln\left( \frac{80}{23} \right )
\]

**Final exact answer:**
\[
\boxed{\ln\left(\frac{80}{23}\right)}
\]

---

**Step 4: Numerical Approximation**

Calculate \( \ln\left(\frac{80}{23}\right) \):

\[
\frac{80}{23} \approx 3.4782608695652174
\]
\[
\ln(3.4782608695652174) \approx 1.2479699653
\]

---

**Step 5: Final JSON Output**

```json
{"answer": "\\ln\\left(\\frac{80}{23}\\right)", "numerical_answer": "1.2479699653"}
```