We start with the integral

  I = ∫₍π/6₎^(π/3) (sin x + cos x)/√(sin 2x) dx.

Step 1. (A Useful Substitution)

Notice that the derivative of (sin x – cos x) is
  d/dx (sin x – cos x) = cos x + sin x.
This exactly matches the numerator. Thus, let

  u = sin x – cos x  ⇒ du = (sin x + cos x) dx.

Now, we need to rewrite the denominator √(sin 2x) in terms of u. Recall that

  sin 2x = 2 sin x cos x.

Also, observe that
  (sin x – cos x)² = sin²x – 2 sin x cos x + cos²x = 1 – 2 sin x cos x.
This shows that
  2 sin x cos x = 1 – (sin x – cos x)² = 1 – u².
Thus,
  √(sin 2x) = √(2 sin x cos x) = √(1 – u²).

Step 2. (Changing the Limits)

We must also change the limits of integration. When x = π/6:
  u = sin(π/6) – cos(π/6) = ½ – (√3)/2 = (1 – √3)/2.
When x = π/3:
  u = sin(π/3) – cos(π/3) = (√3)/2 – ½ = (√3 – 1)/2.

Step 3. (The Transformed Integral)

In terms of u the integral becomes
  I = ∫₍u=(1–√3)/2₎^( (√3–1)/2 ) du/√(1 – u²).

But the antiderivative of 1/√(1 – u²) is arcsin u so that

  I = [arcsin u] evaluated from u=(1–√3)/2 to u=(√3–1)/2.

Thus,
  I = arcsin((√3–1)/2) – arcsin((1–√3)/2).

Notice that (1–√3)/2 = –((√3–1)/2) so using the oddness of the arcsin, we have

  arcsin((1–√3)/2) = –arcsin((√3–1)/2).

Thus,
  I = arcsin((√3–1)/2) – (–arcsin((√3–1)/2))
     = 2·arcsin((√3–1)/2).

This is the exact value of the integral.

Step 4. (Numerical Approximation)

Now, we compute the numerical value. Note that

  (√3 – 1)/2 ≈ (1.7320508075688772 – 1)/2 ≈ 0.3660254037844386.

Then,
  arcsin(0.3660254037844386) ≈ 0.374054 (radians)

so that

  I ≈ 2 × 0.374054 ≈ 0.748108.

Rounded to 10 decimal places the numerical value is 0.7481080000.

Step 5. (Final Answer in JSON Format)

{"answer": "2\\arcsin\\left(\\frac{\\sqrt{3}-1}{2}\\right)", "numerical_answer": "0.7481080000"}