
To solve the definite integral \(\int_{0}^{2} x \arctan\left(\sqrt{x(2-x)}\right) \, dx\), we proceed as follows:

### Step 1: Simplify the argument of the arctangent
First, rewrite the expression inside the square root:
\[
x(2-x) = 2x - x^2 = 1 - (x-1)^2
\]
Thus, \(\sqrt{x(2-x)} = \sqrt{1 - (x-1)^2}\).

### Step 2: Substitution to exploit symmetry
Let \(t = x - 1\), so \(x = t + 1\) and \(dx = dt\). The limits change from \(x=0\) to \(t=-1\) and \(x=2\) to \(t=1\). The integral becomes:
\[
\int_{-1}^{1} (t + 1) \arctan\left(\sqrt{1 - t^2}\right) \, dt
\]
Split this into two integrals:
\[
\int_{-1}^{1} t \arctan\left(\sqrt{1 - t^2}\right) \, dt + \int_{-1}^{1} \arctan\left(\sqrt{1 - t^2}\right) \, dt
\]

### Step 3: Evaluate the first integral (odd function)
The integrand \(t \arctan\left(\sqrt{1 - t^2}\right)\) is an odd function (since \(f(-t) = -f(t)\)). Integrating an odd function over symmetric limits \([-a, a]\) gives zero:
\[
\int_{-1}^{1} t \arctan\left(\sqrt{1 - t^2}\right) \, dt = 0
\]

### Step 4: Evaluate the second integral (even function)
The integrand \(\arctan\left(\sqrt{1 - t^2}\right)\) is even (since \(f(-t) = f(t)\)). Thus:
\[
\int_{-1}^{1} \arctan\left(\sqrt{1 - t^2}\right) \, dt = 2 \int_{0}^{1} \arctan\left(\sqrt{1 - t^2}\right) \, dt
\]

### Step 5: Trigonometric substitution
Let \(t = \sin\theta\), so \(dt = \cos\theta \, d\theta\) and \(\sqrt{1 - t^2} = \cos\theta\). The limits change from \(t=0\) to \(\theta=0\) and \(t=1\) to \(\theta=\pi/2\). The integral becomes:
\[
2 \int_{0}^{\pi/2} \arctan(\cos\theta) \cos\theta \, d\theta
\]

### Step 6: Integration by parts
Let \(u = \arctan(\cos\theta)\) and \(dv = \cos\theta \, d\theta\). Then \(du = \frac{-\sin\theta}{1 + \cos^2\theta} \, d\theta\) and \(v = \sin\theta\). Integration by parts gives:
\[
2 \left[ \left. \arctan(\cos\theta) \sin\theta \right|_{0}^{\pi/2} + \int_{0}^{\pi/2} \frac{\sin^2\theta}{1 + \cos^2\theta} \, d\theta \right]
\]
The boundary term vanishes (since \(\arctan(0) \cdot 1 = 0\) and \(\arctan(1) \cdot 0 = 0\)). Simplify the remaining integral:
\[
2 \int_{0}^{\pi/2} \frac{\sin^2\theta}{1 + \cos^2\theta} \, d\theta = 2 \int_{0}^{\pi/2} \left( \frac{2}{1 + \cos^2\theta} - 1 \right) \, d\theta
\]

### Step 7: Evaluate the remaining integrals
The integral \(\int_{0}^{\pi/2} \frac{1}{1 + \cos^2\theta} \, d\theta\) is a standard result, equal to \(\frac{\pi}{2\sqrt{2}}\). Thus:
\[
2 \left( 2 \cdot \frac{\pi}{2\sqrt{2}} - \frac{\pi}{2} \right) = 2 \left( \frac{\pi}{\sqrt{2}} - \frac{\pi}{2} \right) = \pi\sqrt{2} - \pi
\]

### Final Result
The exact value of the integral is \(\pi(\sqrt{2} - 1)\). The numerical approximation, rounded to 10 decimal places, is approximately \(1.2990381057\).

{"answer": "\(\pi(\sqrt{2} - 1)\)", "numerical_answer": "1.2990381057"}