We wish to evaluate

  I = ∫₀² x cos(√(x(2 – x))) dx.

A good way to attack this integral is first to “center” the x–interval so that the square root becomes a simpler function. In fact, make the substitution

  x = 1 + u       (dx = du),

so that when x = 0 then u = –1 and when x = 2 then u = 1. Also note that

  2 – x = 2 – (1 + u) = 1 – u.
  Thus  x(2 – x) = (1 + u)(1 – u) = 1 – u²   and hence  √(x(2 – x)) = √(1 – u²).

The integral becomes

  I = ∫₋₁¹ (1 + u) cos(√(1 – u²)) du.

Now split the integral into two pieces:

  I = ∫₋₁¹ cos(√(1 – u²)) du + ∫₋₁¹ u cos(√(1 – u²)) du.

Notice that the function cos(√(1 – u²)) is an even function of u (since √(1 – u²) is even) while u is odd. Hence the second integral (the product of an odd and an even function) vanishes. Thus

  I = ∫₋₁¹ cos(√(1 – u²)) du.

Because the integrand is even we can write

  I = 2 ∫₀¹ cos(√(1 – u²)) du.

A trigonometric substitution now makes the square root very nice. Let

  u = cosθ,    so that du = –sinθ dθ.

When u goes from 0 to 1 the angle θ goes from π/2 to 0. (We can reverse the limits.) Also, note that

  √(1 – u²) = √(1 – cos²θ) = sinθ   (for 0 ≤ θ ≤ π/2).
Then

  I = 2 ∫₍θ=π/2₎^(θ=0) cos(sinθ) (–sinθ dθ).

Reversing the limits gives

  I = 2 ∫₀^(π/2) cos(sinθ) sinθ dθ.

It turns out that it is best to “symmetrize” the integration by extending the integration from 0 to π. This can be done by a second substitution. In fact, if instead we make the substitution x = 1 + cosθ (with θ going from π to 0) in the original integral one eventually finds that

  I = ∫₀^(π) sinθ cos(sinθ) dθ.

Now we expand the function cos(sinθ) in a Fourier–Bessel series. One may show (using the standard expansion)

  cos(z sinθ) = J₀(z) + 2∑ₙ₌₁^∞ J₂ₙ(z) cos(2nθ).

Taking z = 1 this gives

  cos(sinθ) = J₀(1) + 2∑ₙ₌₁^∞ J₂ₙ(1) cos(2nθ).

Substituting this into our expression for I we have

  I = ∫₀^(π) sinθ [J₀(1) + 2∑ₙ₌₁^∞ J₂ₙ(1) cos(2nθ)] dθ
    = J₀(1) ∫₀^(π) sinθ dθ + 2∑ₙ₌₁^∞ J₂ₙ(1) ∫₀^(π) sinθ cos(2nθ) dθ.

Now,
  ∫₀^(π) sinθ dθ = 2,
and for each n ≥ 1 the integral
  ∫₀^(π) sinθ cos(2nθ) dθ = 0,
by symmetry. Hence

  I = 2 J₀(1).

Thus the original integral is found in closed‐form in terms of the Bessel function of order zero:

  I = 2J₀(1).

A standard numerical approximation (using, for example, a table or software) gives

  J₀(1) ≈ 0.7651976866,
so that
  I ≈ 2 × 0.7651976866 ≈ 1.5303953732.

Below is the final answer in the required JSON format.

{"answer": "$2J_{0}(1)$", "numerical_answer": "1.5303953732"}