
To solve the definite integral \(\int\limits_0^\infty x^{2-1}e^{-1.0x^2}H_2(1.0x)dx\), we follow these steps:

### Step 1: Simplify the integrand
The integrand is \(x^{2-1}e^{-x^2}H_2(x) = x e^{-x^2}H_2(x)\), where \(H_2(x)\) is the Hermite polynomial of degree 2. The explicit form of \(H_2(x)\) is \(4x^2 - 2\) (derived from the definition of Hermite polynomials). Thus, the integrand becomes:
\[
x e^{-x^2}(4x^2 - 2) = 4x^3 e^{-x^2} - 2x e^{-x^2}
\]

### Step 2: Split the integral into two parts
The integral can be split into two separate integrals:
\[
\int_0^\infty \left(4x^3 e^{-x^2} - 2x e^{-x^2}\right) dx = 4\int_0^\infty x^3 e^{-x^2} dx - 2\int_0^\infty x e^{-x^2} dx
\]

### Step 3: Evaluate the first integral \(4\int_0^\infty x^3 e^{-x^2} dx\)
Use the substitution \(u = x^2\), so \(du = 2x dx\) or \(x dx = \frac{du}{2}\). Then \(x^3 dx = x^2 \cdot x dx = u \cdot \frac{du}{2}\). The integral becomes:
\[
4\int_0^\infty x^3 e^{-x^2} dx = 4 \cdot \frac{1}{2} \int_0^\infty u e^{-u} du = 2 \int_0^\infty u e^{-u} du
\]
The integral \(\int_0^\infty u e^{-u} du\) is the Gamma function \(\Gamma(2) = 1!\) (since \(\Gamma(n) = (n-1)!\) for positive integers \(n\)). Thus:
\[
2 \cdot 1! = 2 \cdot 1 = 2
\]

### Step 4: Evaluate the second integral \(-2\int_0^\infty x e^{-x^2} dx\)
Again, use \(u = x^2\), so \(du = 2x dx\) or \(x dx = \frac{du}{2}\). The integral becomes:
\[
-2\int_0^\infty x e^{-x^2} dx = -2 \cdot \frac{1}{2} \int_0^\infty e^{-u} du = - \int_0^\infty e^{-u} du
\]
The integral \(\int_0^\infty e^{-u} du = 1\), so:
\[
-1
\]

### Step 5: Combine the results
Adding the results of the two integrals:
\[
2 - 1 = 1
\]

### Numerical Approximation
The exact result is \(1\), so the numerical approximation (rounded to 10 decimal places) is \(1.0000000000\).

{"answer": "1", "numerical_answer": "1.0000000000"}