To evaluate the definite integral

$$
\int_0^2 \sqrt{x} \sqrt{2 - x} \cosh\left(\sqrt{x(2 - x)}\right) \, dx,
$$

we begin by observing the structure of the integrand. The product $\sqrt{x} \sqrt{2 - x}$ simplifies to $\sqrt{x(2 - x)}$, and the expression inside the square root becomes symmetric about $x = 1$. This suggests a substitution that centers the interval around 1.

---

### Step 1: Substitution

Let $ t = x - 1 $, so that $ x = t + 1 $, and the limits become $ t \in [-1, 1] $. The integrand becomes:

$$
\sqrt{(t + 1)(1 - t)} \cosh\left(\sqrt{(t + 1)(1 - t)}\right) = \sqrt{1 - t^2} \cosh\left(\sqrt{1 - t^2}\right).
$$

Thus, the integral becomes:

$$
\int_0^2 \sqrt{x} \sqrt{2 - x} \cosh\left(\sqrt{x(2 - x)}\right) dx = \int_{-1}^1 \sqrt{1 - t^2} \cosh\left(\sqrt{1 - t^2}\right) dt.
$$

Since the integrand is even (i.e., symmetric about $t = 0$), we can write:

$$
\int_{-1}^1 \sqrt{1 - t^2} \cosh\left(\sqrt{1 - t^2}\right) dt = 2 \int_0^1 \sqrt{1 - t^2} \cosh\left(\sqrt{1 - t^2}\right) dt.
$$

---

### Step 2: Further Simplification

Let $ u = \sqrt{1 - t^2} $, then $ t = \sqrt{1 - u^2} $, and $ dt = -\frac{u}{\sqrt{1 - u^2}} du $. The limits change from $ t = 0 \to 1 $ to $ u = 1 \to 0 $. The integral becomes:

$$
2 \int_0^1 u \cosh(u) \cdot \frac{u}{\sqrt{1 - u^2}} du = 2 \int_0^1 \frac{u^2 \cosh(u)}{\sqrt{1 - u^2}} du.
$$

This is a known form that can be evaluated in terms of **modified Bessel functions**.

---

### Step 3: Use of Bessel Function Identities

From integral tables or known results, we have:

$$
\int_0^1 \frac{u^2 \cosh(u)}{\sqrt{1 - u^2}} du = \frac{\pi}{4} (I_0(1) + I_1(1)),
$$

where $I_0(x)$ and $I_1(x)$ are the modified Bessel functions of the first kind of order 0 and 1, respectively.

Therefore, the original integral becomes:

$$
2 \cdot \frac{\pi}{4} (I_0(1) + I_1(1)) = \frac{\pi}{2} (I_0(1) + I_1(1)).
$$

---

### Step 4: Numerical Approximation

Using known values of the modified Bessel functions:

- $ I_0(1) \approx 1.2660658777516918 $
- $ I_1(1) \approx 0.565159103992485 $

Adding these:

$$
I_0(1) + I_1(1) \approx 1.8312249817441768
$$

Multiplying by $ \frac{\pi}{2} \approx 1.5707963267948966 $:

$$
\frac{\pi}{2} (I_0(1) + I_1(1)) \approx 1.8312249817441768 \times 1.5707963267948966 \approx 2.8764372843
$$

---

### Final Answer

$$
\boxed{
\left\{
  "answer":