Let's compute the definite integral step by step:

\[
\int_0^1 \left(e^{e^x} - e^{e^x - x}\right) dx
\]

### Step 1: Split the Integral
First, split the integral into two parts:

\[
\int_0^1 e^{e^x} dx - \int_0^1 e^{e^x - x} dx
\]

### Step 2: Simplify the Second Integral
Letâ€™s focus on the second integral:

\[
\int_0^1 e^{e^x - x} dx
\]

Make the substitution \( u = e^x \), so \( du = e^x dx \) and \( dx = \frac{du}{u} \). The limits change from \( x = 0 \) to \( u = 1 \) and \( x = 1 \) to \( u = e \). The integral becomes:

\[
\int_{1}^{e} e^{u - \ln u} \cdot \frac{du}{u} = \int_{1}^{e} e^{u} \cdot e^{-\ln u} \cdot \frac{du}{u} = \int_{1}^{e} e^{u} \cdot \frac{1}{u} \cdot \frac{du}{u} = \int_{1}^{e} \frac{e^{u}}{u^2} du
\]

This doesn't seem immediately helpful, so let's try another approach. Instead, consider integrating by parts for the second integral:

Let \( v = e^{e^x} \) and \( dw = e^{-x} dx \). Then \( dv = e^{e^x} \cdot e^x dx \) and \( w = -e^{-x} \). Applying integration by parts:

\[
\int e^{e^x - x} dx = -e^{-x} e^{e^x} + \int e^{e^x} dx
\]

Thus, the second integral can be written as:

\[
\int_0^1 e^{e^x - x} dx = \left[ -e^{e^x - x} \right]_0^1 + \int_0^1 e^{e^x} dx
\]

### Step 3: Combine the Results
Now, substitute this back into the original expression:

\[
\int_0^1 e^{e^x} dx - \left( \left[ -e^{e^x - x} \right]_0^1 + \int_0^1 e^{e^x} dx \right) = \int_0^1 e^{e^x} dx + \left[ e^{e^x - x} \right]_0^1 - \int_0^1 e^{e^x} dx
\]

The integrals cancel out, leaving:

\[
\left[ e^{e^x - x} \right]_0^1 = e^{e^1 - 1} - e^{e^0 - 0} = e^{e - 1} - e^{1}
\]

### Step 4: Final Answer
The exact value of the integral is:

\[
e^{e - 1} - e
\]

### Step 5: Numerical Approximation
Now, compute the numerical approximation:

\[
e^{e - 1} - e \approx e^{1.7182818285} - e \approx 5.5749415226 - 2.7182818285 \approx 2.8566596941
\]

Rounding to 10 decimal places:

\[
2.8566596941
\]

### Final Answer in JSON
```json
{"answer": "e^{e - 1} - e", "numerical_answer": "2.8566596941"}
```