To solve the definite integral \(\int_0^6 \left( x + (x-3)^7 + \sin(x-3) \right) \, dx\), we will break it down into three separate integrals and solve each one individually.

### Step 1: Break down the integral
\[
\int_0^6 \left( x + (x-3)^7 + \sin(x-3) \right) \, dx = \int_0^6 x \, dx + \int_0^6 (x-3)^7 \, dx + \int_0^6 \sin(x-3) \, dx
\]

### Step 2: Compute each integral separately

#### Integral 1: \(\int_0^6 x \, dx\)
\[
\int_0^6 x \, dx = \left[ \frac{x^2}{2} \right]_0^6 = \frac{6^2}{2} - \frac{0^2}{2} = \frac{36}{2} = 18
\]

#### Integral 2: \(\int_0^6 (x-3)^7 \, dx\)
Let \(u = x - 3\). Then \(du = dx\). When \(x = 0\), \(u = -3\). When \(x = 6\), \(u = 3\).
\[
\int_0^6 (x-3)^7 \, dx = \int_{-3}^3 u^7 \, du
\]
Since \(u^7\) is an odd function, the integral of an odd function over a symmetric interval around zero is zero:
\[
\int_{-3}^3 u^7 \, du = 0
\]

#### Integral 3: \(\int_0^6 \sin(x-3) \, dx\)
Let \(u = x - 3\). Then \(du = dx\). When \(x = 0\), \(u = -3\). When \(x = 6\), \(u = 3\).
\[
\int_0^6 \sin(x-3) \, dx = \int_{-3}^3 \sin u \, du
\]
Since \(\sin u\) is an odd function, the integral of an odd function over a symmetric interval around zero is zero:
\[
\int_{-3}^3 \sin u \, du = 0
\]

### Step 3: Combine the results
\[
\int_0^6 \left( x + (x-3)^7 + \sin(x-3) \right) \, dx = 18 + 0 + 0 = 18
\]

### Step 4: Numerical approximation
The exact answer is already a simple number, so the numerical approximation is the same:
\[
18.0000000000
\]

### Final Answer in JSON format
```json
{"answer": "18", "numerical_answer": "18.0000000000"}
```