
To solve the definite integral \(\int\limits_0^1 \mathbf{L}_0(2\sqrt{x})\mathbf{E}\left(\sqrt{1-x}\right)dx\), we proceed as follows:

### Step 1: Simplify the integrand using properties of Laguerre polynomials
The 0th Laguerre polynomial \(\mathbf{L}_0(x)\) is identically 1 for all \(x\). Thus, the integrand simplifies to \(\mathbf{E}\left(\sqrt{1-x}\right)\). The integral becomes:
\[
\int_0^1 \mathbf{E}\left(\sqrt{1-x}\right) dx
\]

### Step 2: Substitution to simplify the integral
Let \(t = \sqrt{1 - x}\), so \(x = 1 - t^2\) and \(dx = -2t \, dt\). When \(x = 0\), \(t = 1\); when \(x = 1\), \(t = 0\). Reversing the limits of integration, the integral transforms to:
\[
\int_0^1 2t \, \mathbf{E}(t) \, dt
\]

### Step 3: Expand the elliptic integral and interchange integration order
The complete elliptic integral of the second kind \(\mathbf{E}(t)\) is defined as:
\[
\mathbf{E}(t) = \int_0^{\pi/2} \sqrt{1 - t^2 \sin^2\theta} \, d\theta
\]
Substituting this into the integral and interchanging the order of integration (justified by Fubini's theorem), we get:
\[
2 \int_0^{\pi/2} \int_0^1 t \sqrt{1 - t^2 \sin^2\theta} \, dt \, d\theta
\]

### Step 4: Evaluate the inner integral
Let \(u = 1 - t^2 \sin^2\theta\), so \(du = -2t \sin^2\theta \, dt\) and \(t \, dt = -\frac{du}{2 \sin^2\theta}\). The inner integral becomes:
\[
\int_1^{\cos^2\theta} \sqrt{u} \left(-\frac{du}{2 \sin^2\theta}\right) = \frac{1}{2 \sin^2\theta} \int_{\cos^2\theta}^1 \sqrt{u} \, du
\]
Evaluating \(\int \sqrt{u} \, du = \frac{2}{3} u^{3/2}\), we find:
\[
\frac{1}{2 \sin^2\theta} \cdot \frac{2}{3} \left(1 - \cos^3\theta\right) = \frac{1 - \cos^3\theta}{3 \sin^2\theta}
\]

### Step 5: Simplify and evaluate the remaining integral
The integral reduces to:
\[
\frac{2}{3} \int_0^{\pi/2} \frac{1 - \cos^3\theta}{\sin^2\theta} \, d\theta
\]
Using the identity \(1 - \cos^3\theta = (1 - \cos\theta)(1 + \cos\theta + \cos^2\theta)\) and \(\sin^2\theta = (1 - \cos\theta)(1 + \cos\theta)\), we simplify the integrand to:
\[
\frac{1 + \cos\theta + \cos^2\theta}{1 + \cos\theta} = \cos\theta + \frac{1}{1 + \cos\theta}
\]
The integral splits into two parts:
\[
\frac{2}{3} \left( \int_0^{\pi/2} \cos\theta \, d\theta + \int_0^{\pi/2} \frac{1}{1 + \cos\theta} \, d\theta \right)
\]
- The first integral: \(\int_0^{\pi/2} \cos\theta \, d\theta = 1\)
- The second integral: Using \(1 + \cos\theta = 2\cos^2(\theta/2)\), we get \(\int_0^{\pi/2} \frac{1}{1 + \cos\theta} \, d\theta = 1\)

Thus, the total integral is:
\[
\frac{2}{3} (1 + 1) = \frac{4}{3}
\]

### Numerical Approximation
The exact value \(\frac{4}{3}\) is approximately \(1.3333333333\) when rounded to 10 decimal places.

{"answer": "\(\frac{4}{3}\)", "numerical_answer": "1.3333333333"}