Let's denote the integral as
\[
I = \int_0^1 (x-1)^2(x+1)^2(x^2+1)^2(x^4+1)^2\,dx
\]

Let us proceed step by step:

## 1. Simplify the integrand

First, expand (x-1)^2(x+1)^2:
\[
(x-1)^2(x+1)^2 = [(x-1)(x+1)]^2 = (x^2 - 1)^2 = x^4 - 2x^2 + 1
\]

So, the integrand is:
\[
(x^4 - 2x^2 + 1)(x^2 + 1)^2(x^4 + 1)^2
\]

Let's expand \((x^2+1)^2\) and \((x^4+1)^2\):

- \((x^2 + 1)^2 = x^4 + 2x^2 + 1\)
- \((x^4 + 1)^2 = x^8 + 2x^4 + 1\)

So, the full integrand is:
\[
(x^4 - 2x^2 + 1)(x^4 + 2x^2 + 1)(x^8 + 2x^4 + 1)
\]

## 2. Expand (x^4 - 2x^2 + 1)(x^4 + 2x^2 + 1)

Let’s do it:

Let \(a = x^4 - 2x^2 + 1\), \(b = x^4 + 2x^2 + 1\)

\[
ab = (x^4 - 2x^2 + 1)(x^4 + 2x^2 + 1)
\]

Let's multiply term by term:

- \(x^4 \cdot x^4 = x^8\)
- \(x^4 \cdot 2x^2 = 2x^6\)
- \(x^4 \cdot 1 = x^4\)
- \(-2x^2 \cdot x^4 = -2x^6\)
- \(-2x^2 \cdot 2x^2 = -4x^4\)
- \(-2x^2 \cdot 1 = -2x^2\)
- \(1 \cdot x^4 = x^4\)
- \(1 \cdot 2x^2 = 2x^2\)
- \(1 \cdot 1 = 1\)

Sum the like terms:

- \(x^8\)
- \(2x^6 - 2x^6 = 0\)
- \(x^4 - 4x^4 + x^4 = (-2x^4)\)
- \(-2x^2 + 2x^2 = 0\)
- \(+1\)

Thus,
\[
(x^4 - 2x^2 + 1)(x^4 + 2x^2 + 1) = x^8 - 2x^4 + 1
\]

Thus, the integrand simplifies to:
\[
(x^8 - 2x^4 + 1)(x^8 + 2x^4 + 1)
\]

## 3. Final expansion with the remaining factor

Now expand:

Let \(c = x^8 - 2x^4 + 1\), \(d = x^8 + 2x^4 + 1\)

So,
\[
c \cdot d = (x^8 - 2x^4 + 1)(x^8 + 2x^4 + 1)
\]

Multiply term by term:

- \(x^8 \cdot x^8 = x^{16}\)
- \(x^8 \cdot 2x^4 = 2x^{12}\)
- \(x^8 \cdot 1 = x^8\)
- \(-2x^4 \cdot x^8 = -2x^{12}\)
- \(-2x^4 \cdot 2x^4 = -4x^8\)
- \(-2x^4 \cdot 1 = -2x^4\)
- \(1 \cdot x^8 = x^8\)
- \(1 \cdot 2x^4 = 2x^4\)
- \(1 \cdot 1 = 1\)

Sum like terms:

- \(x^{16}\)
- \(2x^{12} - 2x^{12} = 0\)
- \(x^8 - 4x^8 + x^8 = (-2x^8)\)
- \(-2x^4 + 2x^4 = 0\)
- \(+1\)

So:
\[
(x^8 - 2x^4 + 1)(x^8 + 2x^4 + 1) = x^{16} - 2x^8 + 1
\]

Thus,
\[
I = \int_0^1 \left(x^{16} - 2x^8 + 1\right) \, dx
\]

## 4. Integrate term by term

The integral becomes:
\[
I = \int_0^1 x^{16} \, dx - 2\int_0^1 x^8 \, dx + \int_0^1 1 \, dx
\]

Compute the antiderivative of each term from 0 to 1:

- \(\int_0^1 x^{16} dx = \left[\frac{x^{17}}{17}\right]_0^1 = \frac{1}{17}\)
- \(\int_0^1 x^{8} dx = \left[\frac{x^{9}}{9}\right]_0^1 = \frac{1}{9}\)
- \(\int_0^1 1 dx = [x]_0^1 = 1\)

Thus,
\[
I = \frac{1}{17} - 2\cdot\frac{1}{9} + 1 = \frac{1}{17} - \frac{2}{9} + 1
\]

Let’s get the common denominator, \(17\times9 = 153\):

\[
\frac{1}{17} = \frac{9}{153}, \quad \frac{2}{9} = \frac{34}{153}, \quad 1 = \frac{153}{153}
\]
So,
\[
I = \frac{9 - 34 + 153}{153} = \frac{128}{153}
\]

## 5. Numerical Value

Calculate the numerical value, rounded to 10 decimal places:
\[
\frac{128}{153} \approx 0.8366013072
\]

## Final Answer in JSON Format

```json
{"answer": "\\frac{128}{153}", "numerical_answer": "0.8366013072"}
```