To solve the definite integral 

\[
\int_{0}^{1} \frac{1}{1+x^2} \arctan\left(x^{3+\sqrt{8}}\right) dx,
\]

we will follow these steps:

### Step 1: Simplify the Integral
Let’s denote \( \alpha = 3 + \sqrt{8} \). The integral becomes:

\[
I = \int_{0}^{1} \frac{\arctan(x^\alpha)}{1+x^2} dx.
\]

### Step 2: Use Integration by Parts
Let \( u = \arctan(x^\alpha) \), so \( du = \frac{\alpha x^{\alpha-1}}{1 + x^{2\alpha}} dx \).

Let \( dv = \frac{1}{1+x^2} dx \), so \( v = \arctan(x) \).

Using integration by parts \( I = uv \Big|_{0}^{1} - \int_{0}^{1} v du \):

\[
I = \arctan(x^\alpha) \arctan(x) \Big|_{0}^{1} - \int_{0}^{1} \arctan(x) \cdot \frac{\alpha x^{\alpha-1}}{1 + x^{2\alpha}} dx.
\]

At \( x = 0 \), both \( \arctan(x^\alpha) \) and \( \arctan(x) \) are 0. At \( x = 1 \), \( \arctan(1^\alpha) = \arctan(1) = \frac{\pi}{4} \), and \( \arctan(1) = \frac{\pi}{4} \). Thus:

\[
I = \left(\frac{\pi}{4}\right)^2 - \alpha \int_{0}^{1} \frac{x^{\alpha-1} \arctan(x)}{1 + x^{2\alpha}} dx.
\]

### Step 3: Simplify the Remaining Integral
The remaining integral is complicated, but we can exploit symmetry. Let’s consider the substitution \( x = \frac{1}{t} \), \( dx = -\frac{1}{t^2} dt \):

\[
\int_{0}^{1} \frac{x^{\alpha-1} \arctan(x)}{1 + x^{2\alpha}} dx = \int_{\infty}^{1} \frac{(1/t)^{\alpha-1} \arctan(1/t)}{1 + (1/t)^{2\alpha}} \left(-\frac{1}{t^2}\right) dt = \int_{1}^{\infty} \frac{t^{-\alpha+1} \arctan(1/t)}{1 + t^{-2\alpha}} \cdot \frac{1}{t^2} dt.
\]

Simplify the integrand:

\[
\frac{t^{-\alpha+1} \arctan(1/t)}{1 + t^{-2\alpha}} \cdot \frac{1}{t^2} = \frac{t^{-\alpha-1} \arctan(1/t)}{1 + t^{-2\alpha}} = \frac{t^{\alpha-1} \arctan(1/t)}{t^{2\alpha} + 1}.
\]

Now, note that \( \arctan(1/t) = \frac{\pi}{2} - \arctan(t) \). Thus:

\[
\int_{1}^{\infty} \frac{t^{\alpha-1} \left(\frac{\pi}{2} - \arctan(t)\right)}{1 + t^{2\alpha}} dt = \frac{\pi}{2} \int_{1}^{\infty} \frac{t^{\alpha-1}}{1 + t^{2\alpha}} dt - \int_{1}^{\infty} \frac{t^{\alpha-1} \arctan(t)}{1 + t^{2\alpha}} dt.
\]

The first integral can be computed as:

\[
\int_{1}^{\infty} \frac{t^{\alpha-1}}{1 + t^{2\alpha}} dt = \frac{1}{2\alpha} \left[ \ln\left(\frac{1 + t^{2\alpha}}{t^{2\alpha}}\right) \right]_{1}^{\infty} = \frac{1}{2\alpha} \left[ 0 - \ln(2) \right] = -\frac{\ln 2}{2\alpha}.
\]

The second integral is the same as the original integral \( I \) but over \( [1, \infty) \). Combining the two parts:

\[
I = \frac{\pi^2}{16} - \alpha \left( -\frac{\pi \ln 2}{4\alpha} - I \right) = \frac{\pi^2}{16} + \frac{\pi \ln 2}{4} + \alpha I.
\]

Solving for \( I \):

\[
I - \alpha I = \frac{\pi^2}{16} + \frac{\pi \ln 2}{4} \implies I (1 - \alpha) = \frac{\pi^2}{16} + \frac{\pi \ln 2}{4}.
\]

Since \( \alpha = 3 + \sqrt{8} \), \( 1 - \alpha = -2 - \sqrt{8} \). Thus:

\[
I = \frac{\frac{\pi^2}{16} + \frac{\pi \ln 2}{4}}{-2 - \sqrt{8}} = -\frac{\pi^2 + 4 \pi \ln 2}{16 (2 + \sqrt{8})}}.
\]

Simplify \( 2 + \sqrt{8} = 2 + 2\sqrt{2} = 2(1 + \sqrt{2}) \):

\[
I = -\frac{\pi^2 + 4 \pi \ln 2}{32 (1 + \sqrt{2})}}.
\]

Rationalize the denominator:

\[
I = -\frac{(\pi^2 + 4 \pi \ln 2)(1 - \sqrt{2})}{32 (1 - 2)}} = \frac{(\pi^2 + 4 \pi \ln 2)(\sqrt{2} - 1)}{32}}.
\]

### Step 4: Numerical Approximation
Compute the numerical value:

\[
\pi \approx 3.1415926536, \quad \ln 2 \approx 0.6931471806, \quad \sqrt{2} \approx 1.4142135624.
\]

\[
\pi^2 + 4 \pi \ln 2 \approx 9.869604401 + 8.696739277 = 18.566343678.
\]

\[
\sqrt{2} - 1 \approx 0.4142135624.
\]

\[
I \approx \frac{18.566343678 \times 0.4142135624}{32} \approx \frac{7.689214738}{32} \approx 0.2402879606.
\]

Rounding to 10 decimal places:

\[
I \approx 0.2402879606.
\]

### Final Answer
The exact answer is:

\[
I = \frac{(\pi^2 + 4 \pi \ln 2)(\sqrt{2} - 1)}{32}.
\]

The numerical approximation is \( 0.2402879606 \).

```json
{"answer": "\\frac{(\\pi^2 + 4 \\pi \\ln 2)(\\sqrt{2} - 1)}{32}", "numerical_answer": "0.2402879606"}
```