We wish to evaluate

  I = ∫₀² x · arctan(√[x(2 – x)]) dx.

Step 1. A change of variable

It is useful to “center” the interval. Let

  u = x – 1  so that  x = u + 1  and  dx = du.

When x = 0, u = –1 and when x = 2, u = 1. Also note that

  √[x(2 – x)] = √[(u + 1)(2 – (u + 1))]
           = √[(u + 1)(1 – u)]
           = √[1 – u²].

Thus, the integral becomes

  I = ∫ from u = –1 to 1 (u + 1) · arctan(√[1 – u²]) du.

Now split the integrals:
  I = ∫₋₁¹ u · arctan(√[1 – u²]) du + ∫₋₁¹ arctan(√[1 – u²]) du.

The first integrand is an odd function (since u is odd and arctan(√[1 – u²]) is even) so its integral from –1 to 1 is zero. Thus

  I = ∫₋₁¹ arctan(√[1 – u²]) du.

Since the integrand is even, we have

  I = 2 ∫₀¹ arctan(√[1 – u²]) du.

Step 2. A trigonometric substitution

Put u = sinθ. Then when u = 0, θ = 0 and when u = 1, θ = π/2. Also, du = cosθ dθ and
  √[1 – u²] = √[1 – sin²θ] = cosθ  (with cosθ ≥ 0 on [0, π/2]). 

Thus the integral becomes

  I = 2 ∫₀^(π/2) arctan(cosθ) · cosθ dθ.

Let

  A = ∫₀^(π/2) arctan(cosθ) · cosθ dθ,
so that
  I = 2A.

Step 3. Integration by parts

We now evaluate A by parts. Let
  P = arctan(cosθ)  and  dQ = cosθ dθ.
Then
  dP = d/dθ[arctan(cosθ)] dθ = –sinθ/(1 + cos²θ) dθ,
  Q = ∫ cosθ dθ = sinθ.

Integration by parts gives

  A = [P Q]₀^(π/2) – ∫₀^(π/2) Q dP
    = [sinθ · arctan(cosθ)]₀^(π/2) – ∫₀^(π/2) sinθ (– sinθ/(1 + cos²θ)) dθ.
At the endpoints, when θ = π/2, sin(π/2) = 1 and cos(π/2) = 0 so arctan(0) = 0; when θ = 0, sin0 = 0. Thus the boundary term vanishes and

  A = ∫₀^(π/2) sin²θ/(1 + cos²θ) dθ.

Since sin²θ = 1 – cos²θ, write

  A = ∫₀^(π/2) [1 – cos²θ]⁄[1 + cos²θ] dθ
    = ∫₀^(π/2) {1/(1 + cos²θ) – [cos²θ/(1 + cos²θ)]} dθ.

Note that

  cos²θ/(1 + cos²θ) = 1 – 1/(1 + cos²θ),
so that

  A = ∫₀^(π/2) {1/(1 + cos²θ) – [1 – 1/(1 + cos²θ)]} dθ
    = ∫₀^(π/2) [2/(1 + cos²θ) – 1] dθ.

Thus

  A = 2 ∫₀^(π/2) dθ/(1 + cos²θ) – ∫₀^(π/2) dθ  = 2I₁ – (π/2),
  where  I₁ = ∫₀^(π/2) dθ/(1 + cos²θ).

Step 4. Evaluating I₁

To compute I₁, use the substitution u = tanθ. Then
  cosθ = 1/√(1 + u²),  dθ = du/(1 + u²),
and when θ goes from 0 to π/2, u goes from 0 to ∞.

Write cos²θ = 1/(1 + u²) so that

  1 + cos²θ = 1 + 1/(1 + u²) = ( (1+u²) + 1 )/(1+u²) = (u² + 2)/(1 + u²).

Then

  I₁ = ∫₀^(π/2) dθ/(1 + cos²θ)
    = ∫₀^∞ [du/(1 + u²)] · [(1 + u²)/(u² + 2)]
    = ∫₀^∞ du/(u² + 2).

This is a standard integral. Recall that

  ∫₀^∞ du/(u² + a²) = π/(2a).
Here a² = 2 so that a = √2 and

  I₁ = π/(2√2).

Thus,
  A = 2 · [π/(2√2)] – (π/2) = (π/√2) – (π/2).

Now, recalling I = 2A, we have

  I = 2[(π/√2) – (π/2)] = (2π/√2) – π = π(√2 – 1).

Step 5. Final answers

Exact answer in closed‐form:
  I = π(√2 – 1).

For the numerical approximation, note that
  √2 ≈ 1.4142135624  so that  √2 – 1 ≈ 0.4142135624,
and therefore
  I ≈ 3.1415926536 × 0.4142135624 ≈ 1.3012790050.

The final answer in the required JSON format is:
{"answer": "$\\pi(\\sqrt{2}-1)$", "numerical_answer": "1.3012790050"}