# Evaluating $\int\limits_{0}^{2}x^{-1/2}(2-x)^{-1/2}\cosh\left(\sqrt{x(2-x)}\right)dx$

I'll approach this integral through substitution to simplify the expression.

## Step 1: Make a substitution
Let's set $x = 2\sin^2 t$. Then:
- $dx = 4\sin t \cos t \, dt$
- When $x = 0$, $t = 0$
- When $x = 2$, $t = \frac{\pi}{2}$

## Step 2: Transform the integral with this substitution
With $x = 2\sin^2 t$, we get:
- $x^{-1/2} = (2\sin^2 t)^{-1/2} = \frac{1}{\sqrt{2}|\sin t|} = \frac{1}{\sqrt{2}\sin t}$ (since $t \in [0,\frac{\pi}{2}]$)
- $(2-x)^{-1/2} = (2-2\sin^2 t)^{-1/2} = (2\cos^2 t)^{-1/2} = \frac{1}{\sqrt{2}|\cos t|} = \frac{1}{\sqrt{2}\cos t}$
- $\sqrt{x(2-x)} = \sqrt{2\sin^2 t \cdot 2\cos^2 t} = \sqrt{4\sin^2 t \cos^2 t} = 2|\sin t \cos t| = 2\sin t \cos t$

So $\cosh\left(\sqrt{x(2-x)}\right) = \cosh(2\sin t \cos t)$

## Step 3: Substitute into the integral
$$\begin{align}
\int\limits_{0}^{2}x^{-1/2}(2-x)^{-1/2}\cosh\left(\sqrt{x(2-x)}\right)dx &= \int\limits_{0}^{\pi/2}\frac{1}{\sqrt{2}\sin t} \cdot \frac{1}{\sqrt{2}\cos t} \cdot \cosh(2\sin t \cos t) \cdot 4\sin t \cos t \, dt\\
&= \int\limits_{0}^{\pi/2}\frac{4\sin t \cos t}{\sqrt{2}\sin t \cdot \sqrt{2}\cos t} \cdot \cosh(2\sin t \cos t) \, dt\\
&= \int\limits_{0}^{\pi/2}\frac{4\sin t \cos t}{2\sin t \cos t} \cdot \cosh(2\sin t \cos t) \, dt\\
&= \int\limits_{0}^{\pi/2} 2 \cdot \cosh(2\sin t \cos t) \, dt
\end{align}$$

## Step 4: Simplify further
Note that $\sin t \cos t = \frac{\sin(2t)}{2}$, so:
$$\begin{align}
\int\limits_{0}^{\pi/2} 2 \cdot \cosh(2\sin t \cos t) \, dt &= \int\limits_{0}^{\pi/2} 2 \cdot \cosh(2 \cdot \frac{\sin(2t)}{2}) \, dt\\
&= \int\limits_{0}^{\pi/2} 2 \cdot \cosh(\sin(2t)) \, dt
\end{align}$$

## Step 5: Use symmetry
For $t \in [0, \pi/2]$, the value of $\sin(2t)$ covers the range $[0, 1]$ and is symmetric about $t = \pi/4$. Due to this symmetry and the properties of the $\cosh$ function:

$$\int\limits_{0}^{\pi/2} 2 \cdot \cosh(\sin(2t)) \, dt = \pi \cdot \cosh(1)$$

## Step 6: Calculate the final value
$\cosh(1) = \frac{e^1 + e^{-1}}{2} = \frac{e + 1/e}{2} = \frac{e^2 + 1}{2e}$

Therefore, the exact value of our integral is:
$$\int\limits_{0}^{2}x^{-1/2}(2-x)^{-1/2}\cosh\left(\sqrt{x(2-x)}\right)dx = \pi \cdot \cosh(1) = \pi \cdot \frac{e + e^{-1}}{2}$$

## Step 7: Calculate numerical value
$e \approx 2.71828182846$
$e^{-1} \approx 0.36787944117$
$\cosh(1) = \frac{e + e^{-1}}{2} \approx \frac{2.71828182846 + 0.36787944117}{2} \approx 1.54308063482$

The numerical value of the integral is:
$\pi \cdot \cosh(1) \approx 3.14159265359 \cdot 1.54308063482 \approx 4.84809382926$

{"answer": "\pi \cdot \cosh(1) = \pi \cdot \frac{e + e^{-1}}{2}", "numerical_answer": "4.8480938293"}