To solve the definite integral 

\[
\int_{0}^{2} x^{-1/2} (2 - x)^{1/2} \left[1 - 0.5x(2 - x)\right]^{1/2} \, dx,
\]

we proceed with the following steps:

### Step 1: Simplify the Integrand
First, observe the integrand:

\[
x^{-1/2} (2 - x)^{1/2} \left[1 - 0.5x(2 - x)\right]^{1/2}.
\]

Let’s simplify the expression inside the square root:

\[
1 - 0.5x(2 - x) = 1 - x + 0.5x^2 = 0.5x^2 - x + 1.
\]

Notice that:

\[
0.5x^2 - x + 1 = 0.5(x^2 - 2x + 2) = 0.5\left[(x - 1)^2 + 1\right].
\]

Thus, the integrand becomes:

\[
x^{-1/2} (2 - x)^{1/2} \sqrt{0.5\left[(x - 1)^2 + 1\right]}.
\]

### Step 2: Substitution
Let’s make the substitution \( x = 2 \sin^2 \theta \). Then:

\[
dx = 4 \sin \theta \cos \theta \, d\theta,
\]

and the limits change as follows:
- When \( x = 0 \), \( \theta = 0 \).
- When \( x = 2 \), \( \theta = \frac{\pi}{2} \).

Now, express the integrand in terms of \( \theta \):

\[
x^{-1/2} = (2 \sin^2 \theta)^{-1/2} = \frac{1}{\sqrt{2} \sin \theta},
\]

\[
(2 - x)^{1/2} = (2 - 2 \sin^2 \theta)^{1/2} = \sqrt{2} \cos \theta,
\]

\[
0.5x^2 - x + 1 = 0.5(2 \sin^2 \theta)^2 - 2 \sin^2 \theta + 1 = 2 \sin^4 \theta - 2 \sin^2 \theta + 1.
\]

However, this substitution seems to complicate the expression. Let’s try another approach.

### Step 3: Alternative Substitution
Let \( u = \sqrt{x} \), so \( x = u^2 \) and \( dx = 2u \, du \). The limits become:
- When \( x = 0 \), \( u = 0 \).
- When \( x = 2 \), \( u = \sqrt{2} \).

The integrand transforms as:

\[
x^{-1/2} = u^{-1},
\]

\[
(2 - x)^{1/2} = (2 - u^2)^{1/2},
\]

\[
1 - 0.5x(2 - x) = 1 - 0.5u^2(2 - u^2) = 1 - u^2 + 0.5u^4.
\]

Thus, the integral becomes:

\[
\int_{0}^{\sqrt{2}} u^{-1} (2 - u^2)^{1/2} \sqrt{1 - u^2 + 0.5u^4} \cdot 2u \, du = 2 \int_{0}^{\sqrt{2}} (2 - u^2)^{1/2} \sqrt{1 - u^2 + 0.5u^4} \, du.
\]

This still appears complicated. Let’s consider another substitution.

### Step 4: Trigonometric Substitution
Let \( x = 1 + \sin \theta \). Then \( dx = \cos \theta \, d\theta \), and the limits:
- When \( x = 0 \), \( \theta = -\frac{\pi}{2} \).
- When \( x = 2 \), \( \theta = \frac{\pi}{2} \).

The integrand becomes:

\[
x^{-1/2} = (1 + \sin \theta)^{-1/2},
\]

\[
(2 - x)^{1/2} = (1 - \sin \theta)^{1/2},
\]

\[
1 - 0.5x(2 - x) = 1 - 0.5(1 + \sin \theta)(1 - \sin \theta) = 1 - 0.5(1 - \sin^2 \theta) = 0.5 + 0.5 \sin^2 \theta.
\]

Thus, the integral is:

\[
\int_{-\pi/2}^{\pi/2} (1 + \sin \theta)^{-1/2} (1 - \sin \theta)^{1/2} \sqrt{0.5 + 0.5 \sin^2 \theta} \cos \theta \, d\theta.
\]

This seems promising. Notice that:

\[
(1 + \sin \theta)^{-1/2} (1 - \sin \theta)^{1/2} = \sqrt{\frac{1 - \sin \theta}{1 + \sin \theta}} = \sqrt{\frac{(1 - \sin \theta)^2}{1 - \sin^2 \theta}} = \frac{1 - \sin \theta}{\cos \theta},
\]

assuming \( \cos \theta > 0 \). Thus, the integrand simplifies to:

\[
\frac{1 - \sin \theta}{\cos \theta} \sqrt{0.5(1 + \sin^2 \theta)} \cos \theta = (1 - \sin \theta) \sqrt{0.5(1 + \sin^2 \theta)}.
\]

The integral becomes:

\[
\sqrt{0.5} \int_{-\pi/2}^{\pi/2} (1 - \sin \theta) \sqrt{1 + \sin^2 \theta} \, d\theta.
\]

This integral is still non-trivial. Let’s consider the symmetry of the integrand. The term \( \sin \theta \sqrt{1 + \sin^2 \theta} \) is odd, so its integral over \( [-\pi/2, \pi/2] \) is zero. The term \( \sqrt{1 + \sin^2 \theta} \) is even, so the integral simplifies to:

\[
\sqrt{0.5} \cdot 2 \int_{0}^{\pi/2} \sqrt{1 + \sin^2 \theta} \, d\theta = \sqrt{2} \int_{0}^{\pi/2} \sqrt{1 + \sin^2 \theta} \, d\theta.
\]

This is the complete elliptic integral of the second kind \( E(-1) \), where:

\[
E(k) = \int_{0}^{\pi/2} \sqrt{1 - k \sin^2 \theta} \, d\theta.
\]

Thus, our integral is:

\[
\sqrt{2} E(-1).
\]

The value of \( E(-1) \) is known to be:

\[
E(-1) = \frac{\Gamma(1/4)^2}{4 \sqrt{2\pi}} + \frac{\sqrt{\pi} \Gamma(1/4)^2}{4 \Gamma(3/4)^2},
\]

but more commonly, it is recognized that:

\[
E(-1) = \sqrt{2} E\left(\frac{1}{\sqrt{2}}\right) - \frac{\pi}{2 \sqrt{2}},
\]

where \( E\left(\frac{1}{\sqrt{2}}\right) \) is the complete elliptic integral of the second kind evaluated at \( \frac{1}{\sqrt{2}} \). However, for our purposes, we can express the exact answer as:

\[
\sqrt{2} E(-1).
\]

Numerically, \( E(-1) \approx 1.854074677 \), so:

\[
\sqrt{2} E(-1) \approx 1.854074677 \times 1.414213562 \approx 2.622057554.
\]

### Final Answer
The exact answer is \( \sqrt{2} E(-1) \), and the numerical approximation is approximately 2.622057554.

```json
{"answer": "\\sqrt{2} E(-1)", "numerical_answer": "2.6220575543"}
```