# Evaluating $\int\limits_{0}^{\infty}\frac{x^{2}}{e^x-1}\left[2^{3}\sinh\left(0.5x\right)-\sinh\left(0.25x\right)\right]dx$

I'll compute this integral by working with each term separately and using properties of the integral.

## Step 1: Rewrite the integrand
Let's first simplify $2^3\sinh(0.5x) - \sinh(0.25x)$:
$2^3\sinh(0.5x) - \sinh(0.25x) = 8\sinh(0.5x) - \sinh(0.25x)$

So our integral is:
$\int\limits_{0}^{\infty}\frac{x^{2}}{e^x-1}\left[8\sinh\left(0.5x\right)-\sinh\left(0.25x\right)\right]dx$

## Step 2: Apply a known formula
For this type of integral, we can use a result related to Riemann zeta function. For $0 < a < 1$:
$\int\limits_{0}^{\infty}\frac{x^{n}}{e^x-1}\sinh(ax)dx = \Gamma(n+1)\sum_{k=0}^{\infty}\frac{1}{(k+1)^{n+1}}\left[(k+1+a)^{n+1} - (k+1-a)^{n+1}\right]$

When $n=2$, this becomes:
$\int\limits_{0}^{\infty}\frac{x^{2}}{e^x-1}\sinh(ax)dx = 2\sum_{k=0}^{\infty}\frac{1}{(k+1)^{3}}\left[(k+1)a^2 + \frac{a^4}{3}\right]$

Since $\sum_{k=0}^{\infty}\frac{1}{(k+1)^{3}} = \zeta(3)$ and $\sum_{k=0}^{\infty}\frac{1}{(k+1)^{1}} = \zeta(1) = \infty$, we need to use a different approach.

## Step 3: Use the connection to the Hurwitz zeta function
We can express our integral in terms of the zeta function using the relation:
$\int\limits_{0}^{\infty}\frac{x^{n}e^{-ax}}{1-e^{-x}}dx = \Gamma(n+1)\zeta(n+1,a)$

Where $\zeta(s,a)$ is the Hurwitz zeta function.

For our case, we need to transform the integral:
$\frac{x^2}{e^x-1}\sinh(ax) = \frac{x^2}{e^x-1}\frac{e^{ax}-e^{-ax}}{2} = \frac{x^2e^{ax}}{2(e^x-1)} - \frac{x^2e^{-ax}}{2(e^x-1)}$

## Step 4: Apply known results about polygamma functions
For $a > 0$, we have:
$\int\limits_{0}^{\infty}\frac{x^{2}}{e^x-1}\sinh(ax)dx = \frac{\pi^2a}{2} + a^3\left(\frac{\pi^2}{6} + \psi^{(1)}(a)\right)$

Where $\psi^{(1)}(a)$ is the trigamma function.

For our specific integral with $a = 0.5$ and $a = 0.25$:

$\int\limits_{0}^{\infty}\frac{x^{2}}{e^x-1}8\sinh\left(0.5x\right)dx = 8\left[\frac{\pi^2(0.5)}{2} + (0.5)^3\left(\frac{\pi^2}{6} + \psi^{(1)}(0.5)\right)\right]$

$\int\limits_{0}^{\infty}\frac{x^{2}}{e^x-1}\sinh\left(0.25x\right)dx = \frac{\pi^2(0.25)}{2} + (0.25)^3\left(\frac{\pi^2}{6} + \psi^{(1)}(0.25)\right)$

## Step 5: Using special values of the trigamma function
We know that:
- $\psi^{(1)}(0.5) = \frac{\pi^2}{2} - 8G$
- $\psi^{(1)}(0.25) = \frac{\pi^2}{2} + 8G + 2\pi^2$

Where $G ≈ 0.915965594$ is Catalan's constant.

## Step 6: Substituting these values and calculating the result
For the first term:
$8\left[\frac{\pi^2(0.5)}{2} + (0.5)^3\left(\frac{\pi^2}{6} + \psi^{(1)}(0.5)\right)\right]$
$= 8\left[\frac{\pi^2}{4} + \frac{1}{8}\left(\frac{\pi^2}{6} + \frac{\pi^2}{2} - 8G\right)\right]$
$= 8\left[\frac{\pi^2}{4} + \frac{\pi^2}{48} + \frac{\pi^2}{16} - \frac{8G}{8}\right]$
$= 8\left[\frac{12\pi^2}{48} + \frac{\pi^2}{48} + \frac{3\pi^2}{48} - G\right]$
$= 8\left[\frac{16\pi^2}{48} - G\right]$
$= 8\left[\frac{\pi^2}{3} - G\right]$
$= \frac{8\pi^2}{3} - 8G$

For the second term:
$\frac{\pi^2(0.25)}{2} + (0.25)^3\left(\frac{\pi^2}{6} + \psi^{(1)}(0.25)\right)$
$= \frac{\pi^2}{8} + \frac{1}{64}\left(\frac{\pi^2}{6} + \frac{\pi^2}{2} + 8G + 2\pi^2\right)$
$= \frac{\pi^2}{8} + \frac{\pi^2}{384} + \frac{\pi^2}{128} + \frac{8G}{64} + \frac{2\pi^2}{64}$
$= \frac{\pi^2}{8} + \frac{\pi^2}{384} + \frac{3\pi^2}{384} + \frac{G}{8} + \frac{6\pi^2}{192}$
$= \frac{24\pi^2}{192} + \frac{\pi^2}{384} + \frac{3\pi^2}{384} + \frac{G}{8} + \frac{6\pi^2}{192}$
$= \frac{48\pi^2 + 2\pi^2 + 6\pi^2 + 24\pi^2}{384} + \frac{G}{8}$
$= \frac{80\pi^2}{384} + \frac{G}{8}$
$= \frac{5\pi^2}{24} + \frac{G}{8}$

## Step 7: Calculating the full integral
$\int\limits_{0}^{\infty}\frac{x^{2}}{e^x-1}\left[8\sinh\left(0.5x\right)-\sinh\left(0.25x\right)\right]dx$
$= \frac{8\pi^2}{3} - 8G - \left(\frac{5\pi^2}{24} + \frac{G}{8}\right)$
$= \frac{8\pi^2}{3} - 8G - \frac{5\pi^2}{24} - \frac{G}{8}$
$= \frac{64\pi^2}{24} - 8G - \frac{5\pi^2}{24} - \frac{G}{8}$
$= \frac{59\pi^2}{24} - 8G - \frac{G}{8}$
$= \frac{59\pi^2}{24} - \frac{64G + G}{8}$
$= \frac{59\pi^2}{24} - \frac{65G}{8}$

## Step 8: Numerical approximation
$\pi^2 ≈ 9.8696044011$ and $G ≈ 0.915965594177$

$\frac{59\pi^2}{24} - \frac{65G}{8} ≈ \frac{59 \cdot 9.8696044011}{24} - \frac{65 \cdot 0.915965594177}{8}$
$≈ 24.2635074694 - 7.4422204652$
$≈ 16.8212870042$

Therefore, to 10 decimal places, the numerical approximation is $16.8212870042$.

{"answer": "\\frac{59\\pi^2}{24} - \\frac{65G}{8}", "numerical_answer": "16.8212870042"}