# Evaluating $\int_0^\pi\cos(x+\cos(x))\mathrm{d}x$

## Step 1: Analyze the integral

Let's evaluate $I = \int_0^\pi\cos(x+\cos(x))\mathrm{d}x$.

First, I'll make the substitution $u = \pi - x$. This gives:
- $x = \pi - u$
- $dx = -du$
- When $x = 0$, $u = \pi$
- When $x = \pi$, $u = 0$

So the integral becomes:
$I = \int_\pi^0\cos((\pi-u)+\cos(\pi-u))(-du)$
$I = \int_0^\pi\cos(\pi-u+\cos(\pi-u))du$

Since $\cos(\pi-u) = -\cos(u)$, we have:
$I = \int_0^\pi\cos(\pi-u-\cos(u))du$
$I = \int_0^\pi\cos(\pi-(u+\cos(u)))du$

Using the property $\cos(\pi-\theta) = -\cos(\theta)$:
$I = \int_0^\pi-\cos(u+\cos(u))du$
$I = -\int_0^\pi\cos(u+\cos(u))du$

But this is just $-I$, which means:
$I = -I$
$2I = 0$
$I = 0$

## Step 2: Verification using symmetry

We can verify this result by examining the behavior of the function $f(x) = \cos(x+\cos(x))$ in the interval $[0,\pi]$.

If we can show that $f(\pi-x) = -f(x)$ for all $x \in [0,\pi]$, then the integral must be zero due to symmetry.

For $f(\pi-x)$:
$f(\pi-x) = \cos((\pi-x)+\cos(\pi-x))$
$= \cos(\pi-x-\cos(x))$
$= \cos(\pi-(x+\cos(x)))$
$= -\cos(x+\cos(x))$
$= -f(x)$

This confirms our result: the function is odd about $x = \pi/2$, so its integral over $[0,\pi]$ is zero.

## Step 3: Numerical approximation

The exact value of the integral is 0.

Numerically, this is 0.0000000000 (rounded to 10 decimal places).

## Final Answer

{"answer": "0", "numerical_answer": "0.0000000000"}