To solve the definite integral \(\int_{\frac{1}{8}}^{\frac{1}{4}} \frac{\ln(2x) \ln(4x) \ln(8x)}{x} \, dx\), we proceed as follows:

1. **Substitution and Simplification**:
   - Let \( t = \ln x \). Then, \( dt = \frac{1}{x} dx \), transforming the integral into:
     \[
     \int_{t_1}^{t_2} (\ln 2 + t)(2\ln 2 + t)(3\ln 2 + t) \, dt
     \]
   - The limits of integration change from \( x = \frac{1}{8} \) to \( t = -3\ln 2 \) and from \( x = \frac{1}{4} \) to \( t = -2\ln 2 \).

2. **Expansion of the Integrand**:
   - Let \( a = \ln 2 \). The integrand becomes:
     \[
     (a + t)(2a + t)(3a + t)
     \]
   - Expanding this product step-by-step results in:
     \[
     t^3 + 6a t^2 + 11a^2 t + 6a^3
     \]

3. **Integration**:
   - Integrate term-by-term:
     \[
     \int (t^3 + 6a t^2 + 11a^2 t + 6a^3) \, dt = \frac{1}{4}t^4 + 2a t^3 + \frac{11}{2}a^2 t^2 + 6a^3 t
     \]

4. **Evaluation of the Definite Integral**:
   - Evaluate the antiderivative at the limits \( t = -2a \) and \( t = -3a \):
     - At \( t = -2a \):
       \[
       \frac{1}{4}(-2a)^4 + 2a(-2a)^3 + \frac{11}{2}a^2(-2a)^2 + 6a^3(-2a) = -2a^4
       \]
     - At \( t = -3a \):
       \[
       \frac{1}{4}(-3a)^4 + 2a(-3a)^3 + \frac{11}{2}a^2(-3a)^2 + 6a^3(-3a) = -\frac{9}{4}a^4
       \]
   - Subtract the results:
     \[
     -2a^4 - \left(-\frac{9}{4}a^4\right) = \frac{1}{4}a^4
     \]
   - Substituting \( a = \ln 2 \), the exact answer is:
     \[
     \frac{(\ln 2)^4}{4}
     \]

5. **Numerical Approximation**:
   - Using \( \ln 2 \approx 0.69314718056 \), we compute:
     \[
     \frac{(\ln 2)^4}{4} \approx \frac{0.23083509866}{4} \approx 0.0577087747
     \]

Final Answer:
\[
\boxed{"answer": "\\frac{(\\ln 2)^4}{4}", "numerical_answer": "0.0577087747"}
\]