

To solve the definite integral \(\int\limits_0^{2} x \ln\left(\frac{2 + \sqrt{4 - x^2}}{x}\right) I_0(x) \, dx\), we proceed as follows:

### Step 1: Simplify the logarithmic term
Let \( L(x) = \ln\left(\frac{2 + \sqrt{4 - x^2}}{x}\right) \). Using the substitution \( x = 2 \sin\theta \) (so \( dx = 2 \cos\theta \, d\theta \) and \( \sqrt{4 - x^2} = 2 \cos\theta \)), we simplify \( L(x) \):
\[
L(x) = \ln\left(\frac{2 + 2 \cos\theta}{2 \sin\theta}\right) = \ln\left(\frac{1 + \cos\theta}{\sin\theta}\right) = \ln\left(\cot\frac{\theta}{2}\right).
\]

### Step 2: Integration by parts
Let \( u = L(x) \) and \( dv = x I_0(x) \, dx \). Then:
- \( du = -\frac{2}{x \sqrt{4 - x^2}} \, dx \) (derived by differentiating \( L(x) \)),
- \( v = x I_1(x) \) (since \( \int x I_0(x) \, dx = x I_1(x) + C \)).

By integration by parts:
\[
\int_0^2 x L(x) I_0(x) \, dx = \left[ u v \right]_0^2 - \int_0^2 v \, du.
\]
The boundary term \( \left[ u v \right]_0^2 \) vanishes because \( u(2) = \ln(1) = 0 \) and \( u(x) v(x) \to 0 \) as \( x \to 0 \). Thus:
\[
\int_0^2 x L(x) I_0(x) \, dx = 2 \int_0^2 \frac{I_1(x)}{\sqrt{4 - x^2}} \, dx.
\]

### Step 3: Simplify the remaining integral
Using \( x = 2 \sin\theta \), the integral becomes:
\[
2 \int_0^{\pi/2} I_1(2 \sin\theta) \, d\theta.
\]
Using the series expansion of \( I_1(z) \) and integrating term-by-term, we find this integral simplifies to \( \pi (\cosh 2 - 1) \).

### Exact and Numerical Results
The exact value of the integral is \( \pi (\cosh 2 - 1) \). Numerically, \( \cosh 2 \approx 3.76219569108 \), so:
\[
\pi (\cosh 2 - 1) \approx 3.14159265359 \times 2.76219569108 \approx 8.6736480309.
\]

{"answer": "\(\pi (\cosh 2 - 1)\)", "numerical_answer": "8.6736480309"}