Let's solve the integral:
\[
I = \int_{0}^{2} x^{-1/2} H_{3}\left( \sqrt[4]{x(2-x)} \right) \, dx
\]
where \( H_3(x) = 8x^3 - 12x \) is the third Hermite polynomial.

---

**Step 1: Substitute and simplify the integrand**

Let us first expand \( H_3 \) at the argument \( y = \sqrt[4]{x(2-x)} \):

\[
H_3 \left( \sqrt[4]{x(2-x)} \right)
= 8 \left( \sqrt[4]{x(2-x)} \right)^3 - 12 \left( \sqrt[4]{x(2-x)} \right)
\]

Recalling \( (\sqrt[4]{x(2-x)})^3 = [x(2-x)]^{3/4} \) and \( (\sqrt[4]{x(2-x)}) = [x(2-x)]^{1/4} \):

\[
H_3 \left( \sqrt[4]{x(2-x)} \right)
= 8 [x(2-x)]^{3/4} - 12 [x(2-x)]^{1/4}
\]

So the integrand is:
\[
x^{-1/2} \left( 8[x(2-x)]^{3/4} - 12[x(2-x)]^{1/4} \right)
= 8 x^{-1/2} [x(2-x)]^{3/4} - 12 x^{-1/2} [x(2-x)]^{1/4}
\]

Now,
\[
x^{-1/2} [x(2-x)]^{a} = x^{-1/2} x^{a} (2-x)^{a} = x^{a-1/2} (2-x)^{a}
\]
So, write as:
\[
I = 8 \int_0^2 x^{(3/4) - (1/2)} (2-x)^{3/4} dx - 12 \int_0^2 x^{(1/4)-(1/2)} (2-x)^{1/4} dx
\]
\[
= 8 \int_0^2 x^{1/4} (2-x)^{3/4} dx - 12 \int_0^2 x^{-1/4} (2-x)^{1/4} dx
\]

---

**Step 2: Change of variable**

Let's use the substitution \( x = 2t \), \( dx = 2dt \), with \( x \in [0,2] \implies t \in [0,1] \):

Now,
- \( x = 2t \)
- \( 2-x = 2(1-t) \)

This gives:

\[
I = 8 \int_0^2 x^{1/4} (2-x)^{3/4} dx - 12 \int_0^2 x^{-1/4} (2-x)^{1/4} dx
\]
Substitute:

1st term:
\[
\int_0^2 x^{1/4} (2-x)^{3/4} dx = \int_{t=0}^{t=1} (2t)^{1/4} [2(1-t)]^{3/4} 2 dt
\]
\[
= 2 \int_{0}^1 (2t)^{1/4} [2(1-t)]^{3/4} dt
\]
\[
= 2 \int_{0}^{1} (2)^{1/4} t^{1/4} (2)^{3/4} (1-t)^{3/4} dt
\]
\[
= 2 (2^{1/4+3/4}) \int_{0}^{1} t^{1/4} (1-t)^{3/4} dt
\]
\[
= 2 \cdot 2^{1} \int_{0}^1 t^{1/4} (1-t)^{3/4} dt
= 4 \int_{0}^1 t^{1/4} (1-t)^{3/4} dt
\]

2nd term:
\[
\int_0^2 x^{-1/4} (2-x)^{1/4} dx
= \int_{0}^{1} (2t)^{-1/4} [2(1-t)]^{1/4} 2 dt
\]
\[
= 2 (2t)^{-1/4} [2(1-t)]^{1/4} dt
= 2 \cdot 2^{-1/4} t^{-1/4} 2^{1/4} (1-t)^{1/4} dt
= 2 \cdot t^{-1/4}(1-t)^{1/4} dt
\]

So the second term is:
\[
= 2 \int_0^1 t^{-1/4} (1-t)^{1/4} dt
\]

So overall,
\[
I = 8 \cdot [4 \int_0^1 t^{1/4}(1-t)^{3/4} dt ] - 12 \cdot [2 \int_0^1 t^{-1/4}(1-t)^{1/4} dt]
= 32 \int_0^1 t^{1/4}(1-t)^{3/4} dt - 24 \int_0^1 t^{-1/4}(1-t)^{1/4} dt
\]

---

**Step 3: Express as Beta functions**

The Beta function is defined as
\[
B(a,b) = \int_0^1 t^{a-1}(1-t)^{b-1} dt
\]

So,
\[
\int_0^1 t^{1/4}(1-t)^{3/4}\,dt = B(1+1/4, 1+3/4) = B(5/4, 7/4)
\]
\[
\int_0^1 t^{-1/4}(1-t)^{1/4}\,dt = B(1-1/4, 1+1/4) = B(3/4, 5/4)
\]

Therefore,
\[
I = 32 B\left(\frac{5}{4}, \frac{7}{4}\right) - 24 B\left(\frac{3}{4},\frac{5}{4}\right)
\]

Recall:
\[
B(a, b) = \frac{\Gamma(a)\Gamma(b)}{\Gamma(a+b)}
\]

So, the exact answer is:
\[
I = 32 \frac{\Gamma(5/4) \Gamma(7/4)}{\Gamma(3)} - 24 \frac{\Gamma(3/4)\Gamma(5/4)}{\Gamma(2)}
\]
Now, \( \Gamma(3) = 2! = 2 \), \( \Gamma(2) = 1! = 1 \):

So,
\[
I = 16\, \Gamma\left(\frac{5}{4}\right) \Gamma\left(\frac{7}{4}\right) - 24\, \Gamma\left(\frac{3}{4}\right) \Gamma\left(\frac{5}{4}\right)
\]

Or, factored:
\[
I = \Gamma\left(\frac{5}{4}\right) \left[ 16\, \Gamma\left(\frac{7}{4}\right) - 24\, \Gamma\left(\frac{3}{4}\right) \right]
\]

---

**Step 4: Numerical approximation**

Let's evaluate:

- \( \Gamma(5/4) \)
- \( \Gamma(7/4) \)
- \( \Gamma(3/4) \)

Use known values (from mathematical tables or Mathematica):
- \( \Gamma(5/4) \approx 0.9064024770554770 \)
- \( \Gamma(7/4) \approx 1.2254167024651776 \)
- \( \Gamma(3/4) \approx 1.2254167024651776 \)

Wait, let's double check:
- \( \Gamma(1.25) \approx 0.9064024770554770 \)
- \( \Gamma(1.75) \approx 0.9181687423997606 \)
- \( \Gamma(0.75) \approx 1.2254167024651776 \)

So,
- \( \Gamma(5/4) \approx 0.9064024770554770 \)
- \( \Gamma(7/4) \approx 0.9181687423997606 \)
- \( \Gamma(3/4) \approx 1.2254167024651776 \)

Compute:
\[
16 \times \Gamma(7/4) = 16 \times 0.9181687423997606 = 14.69069987839617
\]
\[
24 \times \Gamma(3/4) = 24 \times 1.2254167024651776 = 29.40996085916426
\]
\[
\text{Difference: } 14.69069987839617 - 29.40996085916426 = -14.71926098076809
\]
\[
I = \Gamma(5/4) \times (-14.71926098076809)
\]
\[
= 0.9064024770554770 \times (-14.71926098076809) = -13.3456249529
\]

Let's carry out the computation precisely:

\[
0.9064024770554770 \times (-14.71926098076809) = -13.345624952977214
\]

---

**Step 5: Final answers**

- **Exact answer:**
\[
I = \Gamma\left( \frac{5}{4} \right) \left[ 16 \Gamma\left( \frac{7}{4} \right) - 24 \Gamma\left( \frac{3}{4} \right) \right]
\]
or more expanded:
\[
I = 16\,\Gamma\left(\frac{5}{4}\right)\Gamma\left(\frac{7}{4}\right) - 24\,\Gamma\left(\frac{5}{4}\right)\Gamma\left(\frac{3}{4}\right)
\]

- **Numerical answer:**
\[
I \approx -13.3456249530
\]
(rounded to 10 decimal places)

---

**JSON output**

```json
{"answer": "16\\,\\Gamma\\left(\\frac{5}{4}\\right) \\Gamma\\left(\\frac{7}{4}\\right) - 24\\,\\Gamma\\left(\\frac{5}{4}\\right) \\Gamma\\left(\\frac{3}{4}\\right)", "numerical_answer": "-13.3456249530"}
```