
To solve the definite integral \(\int\limits_0^{2} x^{1/2}(2 - x)^{1/2}\cos\left(\sqrt{x(2 - x)}\right)dx\), we proceed as follows:

### Step 1: Substitution and Simplification
First, observe that \(x(2 - x) = 1 - (x - 1)^2\), suggesting a trigonometric substitution. Let \(x = 1 + \sin\theta\), so \(dx = \cos\theta d\theta\). The limits of integration transform as \(x = 0 \to \theta = -\pi/2\) and \(x = 2 \to \theta = \pi/2\). The term \(\sqrt{x(2 - x)}\) simplifies to \(\cos\theta\) (since \(x(2 - x) = 1 - \sin^2\theta = \cos^2\theta\)), and the integrand becomes:
\[
\sqrt{x(2 - x)}\cos\left(\sqrt{x(2 - x)}\right)dx = \cos\theta \cdot \cos(\cos\theta) \cdot \cos\theta d\theta = \cos^2\theta \cos(\cos\theta) d\theta
\]
The integral thus transforms to:
\[
\int_{-\pi/2}^{\pi/2} \cos^2\theta \cos(\cos\theta) d\theta
\]
By symmetry, this is \(2\int_0^{\pi/2} \cos^2\theta \cos(\cos\theta) d\theta\).

### Step 2: Using Bessel Function Integral Representations
The integral involves \(\cos(\cos\theta)\), which relates to Bessel functions. Recall that the Bessel function of the first kind \(J_0(z)\) has the integral representation:
\[
J_0(z) = \frac{1}{\pi} \int_0^\pi \cos(z \cos\theta) d\theta
\]
For \(z = 1\), this gives \(\int_0^\pi \cos(\cos\theta) d\theta = \pi J_0(1)\). Similarly, using Fourier series expansions, the integral \(\int_0^\pi \cos(2\theta) \cos(\cos\theta) d\theta\) relates to \(J_2(1)\). 

### Step 3: Evaluating the Integral
Expanding \(\cos^2\theta = \frac{1 + \cos(2\theta)}{2}\), the integral becomes:
\[
2\int_0^{\pi/2} \cos^2\theta \cos(\cos\theta) d\theta = \int_0^{\pi/2} (1 + \cos(2\theta)) \cos(\cos\theta) d\theta
\]
Using symmetry and Bessel function properties, this simplifies to:
\[
\frac{\pi}{2} \left( J_0(1) - J_2(1) \right)
\]

### Step 4: Numerical Approximation
Using known values of Bessel functions:
- \(J_0(1) \approx 0.7651976865579666\)
- \(J_2(1) \approx 0.11490348493190048\)

Thus:
\[
\frac{\pi}{2} \left( J_0(1) - J_2(1) \right) \approx \frac{\pi}{2} (0.7651976865579666 - 0.11490348493190048) \approx 1.021734438
\]

### Final Answer
The exact answer is \(\frac{\pi}{2} \left( J_0(1) - J_2(1) \right)\), and the numerical approximation is approximately \(1.021734438\).

{"answer": "\\frac{\\pi}{2} \\left( J_0(1) - J_2(1) \\right)", "numerical_answer": "1.0217344380"}