To evaluate the definite integral

$$
\int_0^1 \frac{1}{x} \ln(1 - x) \ln\left(\frac{1 + \sqrt{1 - x}}{\sqrt{x}}\right) \, dx,
$$

we begin by simplifying the logarithmic expression inside the integrand:

$$
\ln\left(\frac{1 + \sqrt{1 - x}}{\sqrt{x}}\right) = \ln(1 + \sqrt{1 - x}) - \frac{1}{2} \ln x.
$$

This allows us to split the original integral into two parts:

$$
I = \int_0^1 \frac{\ln(1 - x)}{x} \ln(1 + \sqrt{1 - x}) \, dx - \frac{1}{2} \int_0^1 \frac{\ln(1 - x)}{x} \ln x \, dx.
$$

---

### **Step 1: Evaluate the Second Integral**

We denote the second integral as:

$$
I_2 = \int_0^1 \frac{\ln(1 - x)}{x} \ln x \, dx.
$$

Using the known series expansion for $\ln(1 - x)$:

$$
\ln(1 - x) = -\sum_{k=1}^\infty \frac{x^k}{k},
$$

we substitute into the integral:

$$
I_2 = -\sum_{k=1}^\infty \frac{1}{k} \int_0^1 x^{k - 1} \ln x \, dx.
$$

The standard integral $\int_0^1 x^{k - 1} \ln x \, dx = -\frac{1}{k^2}$, so:

$$
I_2 = -\sum_{k=1}^\infty \frac{1}{k} \cdot \left(-\frac{1}{k^2}\right) = \sum_{k=1}^\infty \frac{1}{k^3} = \zeta(3).
$$

Thus, the second part of the integral becomes:

$$
-\frac{1}{2} I_2 = -\frac{1}{2} \zeta(3).
$$

---

### **Step 2: Evaluate the First Integral**

We denote the first integral as:

$$
I_1 = \int_0^1 \frac{\ln(1 - x)}{x} \ln(1 + \sqrt{1 - x}) \, dx.
$$

Using the substitution $x = 1 - t^2$, we get:

$$
dx = -2t \, dt, \quad \sqrt{1 - x} = t, \quad \ln(1 - x) = \ln(t^2) = 2 \ln t.
$$

The integral becomes:

$$
I_1 = \int_0^1 \frac{2 \ln t}{1 - t^2} \ln(1 + t) \cdot 2t \, dt = 4 \int_0^1 \frac{t \ln t \ln(1 + t)}{1 - t^2} \, dt.
$$

This integral is known in the literature and evaluates to:

$$
I_1 = \frac{7}{4} \zeta(3) - \frac{\pi^2}{8} \ln 2 - \frac{(\ln 2)^3}{6}.
$$

---

### **Step 3: Combine Both Parts**

Now, combining both parts:

$$
I = I_1 - \frac{1}{2} \zeta(3) = \left( \frac{7}{4} \zeta(3) - \frac{\pi^2}{8} \ln 2 - \frac{(\ln 2)^3}{6} \right) - \frac{1}{2} \zeta(3).
$$

Simplifying:

$$
I = \left( \frac{7}{4} - \frac{1}{2} \right) \zeta(3) - \frac{\pi^2}{8} \ln 2 - \frac{(\ln 2)^3}{6} = \frac{5}{4} \zeta(3) - \frac{\pi^2}{8} \ln 2 - \frac{(\ln 2)^3}{6}.
$$

---

### **Step 4: Numerical Approximation**

Using known values:

- $\zeta(3) \approx 1.