To solve the definite integral \(\int\limits_0^{2.0} x^{-1/2} \left[1 + \sqrt{x(2.0 - x)}\right]^{-3/2} \, dx\), we proceed as follows:

1. **Substitution**: Let \(x - 1 = \sin\theta\). This transforms the integral limits from \(x = 0\) to \(x = 2\) into \(\theta = -\pi/2\) to \(\theta = \pi/2\). The integral becomes:
   \[
   \int_{-\pi/2}^{\pi/2} (1 + \sin\theta)^{-1/2} \left[1 + \cos\theta\right]^{-3/2} \cos\theta \, d\theta
   \]

2. **Trigonometric Identities**: Using \(1 + \cos\theta = 2\cos^2(\theta/2)\) and \(1 + \sin\theta = (\sin(\theta/2) + \cos(\theta/2))^2\), the integrand simplifies to:
   \[
   2^{-3/2} \int_{-\pi/2}^{\pi/2} \frac{\cos\theta}{(\sin(\theta/2) + \cos(\theta/2)) \cos^3(\theta/2)} \, d\theta
   \]

3. **Substitution \(\phi = \theta/2\)**: Changing variables to \(\phi = \theta/2\) with \(d\theta = 2d\phi\) and adjusting limits from \(-\pi/4\) to \(\pi/4\), the integral becomes:
   \[
   2^{-1/2} \int_{-\pi/4}^{\pi/4} \frac{\cos(2\phi)}{(\sin\phi + \cos\phi) \cos^3\phi} \, d\phi
   \]

4. **Further Substitution \(t = \phi + \pi/4\)**: This shifts the limits to \(0\) and \(\pi/2\). Simplifying using trigonometric identities, the integral reduces to:
   \[
   2\sqrt{2} \int_{0}^{\pi/2} \frac{\cos t}{(\cos t + \sin t)^3} \, dt
   \]

5. **Final Substitution \(u = \tan t\)**: Transforming the integral into:
   \[
   2\sqrt{2} \int_{0}^{\infty} \frac{1}{(1 + u)^3} \, du = 2\sqrt{2} \left[ \frac{1}{2} \right] = \sqrt{2}
   \]

The exact value of the integral is \(\sqrt{2}\). Numerically, this approximates to \(1.4142135624\) when rounded to 10 decimal places.

```json
{"answer": "\\sqrt{2}", "numerical_answer": "1.4142135624"}
```