
To solve the definite integral \(\int\limits_0^4 x^{-1/2}(4-x)^{-1/2}[1-0.25x(4-x)]^{1/2}dx\), we proceed as follows:

### Step 1: Simplify the integrand
First, simplify the term inside the square root:
\[
1 - 0.25x(4 - x) = 1 - x + 0.25x^2 = (0.5x - 1)^2
\]
Thus, the square root term becomes \(|0.5x - 1|\). The integrand simplifies to:
\[
x^{-1/2}(4 - x)^{-1/2} \cdot |0.5x - 1|
\]

### Step 2: Substitution
Let \(x = 4t\), so \(dx = 4dt\). When \(x = 0\), \(t = 0\); when \(x = 4\), \(t = 1\). Substituting:
\[
x^{-1/2} = (4t)^{-1/2} = \frac{1}{2}t^{-1/2}, \quad (4 - x)^{-1/2} = (4 - 4t)^{-1/2} = \frac{1}{2}(1 - t)^{-1/2}
\]
The product \(x^{-1/2}(4 - x)^{-1/2}\) becomes \(\frac{1}{4}t^{-1/2}(1 - t)^{-1/2}\). The term \(|0.5x - 1| = |2t - 1|\). The integral transforms to:
\[
\int_0^1 t^{-1/2}(1 - t)^{-1/2} \cdot |2t - 1| \cdot 4 \cdot \frac{1}{4} dt = \int_0^1 t^{-1/2}(1 - t)^{-1/2} |2t - 1| dt
\]

### Step 3: Split the integral
The absolute value \(|2t - 1|\) changes sign at \(t = 1/2\). Split the integral into two parts:
\[
\int_0^{1/2} t^{-1/2}(1 - t)^{-1/2}(1 - 2t) dt + \int_{1/2}^1 t^{-1/2}(1 - t)^{-1/2}(2t - 1) dt
\]

### Step 4: Evaluate the integrals
Using the substitution \(t = \sin^2\theta\) (so \(dt = 2\sin\theta\cos\theta d\theta\)), the first integral transforms to the second integral (by symmetry). Evaluating the second integral:
\[
\int_{1/2}^1 t^{-1/2}(1 - t)^{-1/2}(2t - 1) dt = 1
\]
Thus, the total integral is \(2 \times 1 = 2\).

### Numerical Approximation
The exact value is \(2\), so the numerical approximation is \(2.0000000000\).

{"answer": "2", "numerical_answer": "2.0000000000"}