Let's evaluate the definite integral:
\[
I = \int_0^1 \frac{1}{x} \arccos x \, \arcsin^2 x \, dx
\]

### Step 1: Substitution

Let us use the substitution \( x = \sin \theta \), where \( \theta \) goes from \( 0 \) to \( \frac{\pi}{2} \):

- \( dx = \cos\theta\, d\theta \)
- \( \arccos x = \arccos(\sin\theta) = \frac{\pi}{2} - \theta \)
- \( \arcsin x = \theta \), so \( \arcsin^2 x = \theta^2 \)
- When \( x = 0 \), \( \theta = 0 \); when \( x = 1 \), \( \theta = \frac{\pi}{2} \)

Expressing the integrand in terms of \( \theta \):

\[
I = \int_{x=0}^{x=1} \frac{1}{x} \arccos x \arcsin^2 x \, dx =
\int_{\theta=0}^{\theta=\frac{\pi}{2}} \frac{1}{\sin\theta} \left(\frac{\pi}{2} - \theta\right) \theta^2 \cos\theta \, d\theta
\]

Now, \(\frac{\cos\theta}{\sin\theta} = \cot\theta\), so

\[
I = \int_0^{\frac{\pi}{2}} \left(\frac{\pi}{2} - \theta\right) \theta^2 \cot\theta \, d\theta
\]

### Step 2: Expand the integrand

\[
I = \frac{\pi}{2} \int_0^{\frac{\pi}{2}} \theta^2 \cot\theta\, d\theta - \int_0^{\frac{\pi}{2}} \theta^3 \cot\theta\, d\theta
\]

Let us define:
- \( I_1 = \int_0^{\frac{\pi}{2}} \theta^2 \cot\theta\, d\theta \)
- \( I_2 = \int_0^{\frac{\pi}{2}} \theta^3 \cot\theta\, d\theta \)
So:
\[
I = \frac{\pi}{2} I_1 - I_2
\]

#### Compute \( I_1 \):

We use integration by parts with:
- \( u = \theta^2 \), \( dv = \cot\theta\, d\theta \)
- \( du = 2\theta\, d\theta \), \( v = \log\sin\theta \)

\[
I_1 = \left[ \theta^2 \log\sin\theta \right]_0^{\frac{\pi}{2}} - \int_0^{\frac{\pi}{2}} 2\theta \log\sin\theta\, d\theta
\]

As \(\theta\to 0\), \(\log\sin\theta \sim \log\theta\), so \(\theta^2 \log\sin\theta \to 0\).
At \(\theta = \frac{\pi}{2}\), \(\log\sin(\frac{\pi}{2}) = \log 1 = 0\).

Thus, the boundary term vanishes and:

\[
I_1 = -2 \int_0^{\frac{\pi}{2}} \theta \log\sin\theta\, d\theta
\]

Let’s denote:

\[
J_1 = \int_0^{\frac{\pi}{2}} \theta \log\sin\theta\, d\theta
\]
So:
\[
I_1 = -2 J_1
\]

#### Compute \( I_2 \):

Similarly, use integration by parts:
- \( u = \theta^3 \), \( dv = \cot\theta\, d\theta \)
- \( du = 3\theta^2\, d\theta \), \( v = \log\sin\theta \)

\[
I_2 = \left[ \theta^3 \log\sin\theta \right]_0^{\frac{\pi}{2}} - \int_0^{\frac{\pi}{2}} 3\theta^2 \log\sin\theta\, d\theta
\]
Boundary term vanishes as above:

\[
I_2 = -3 \int_0^{\frac{\pi}{2}} \theta^2 \log\sin\theta\, d\theta
\]

Let’s denote:

\[
J_2 = \int_0^{\frac{\pi}{2}} \theta^2 \log\sin\theta\, d\theta
\]
So:
\[
I_2 = -3 J_2
\]

#### Go back to \(I\):

\[
I = \frac{\pi}{2} I_1 - I_2 = \frac{\pi}{2} (-2 J_1) - (-3 J_2) = -\pi J_1 + 3 J_2
\]

### Step 3: Find \( J_1 \) and \( J_2 \):

Recall:
\[
J_n = \int_0^{\frac{\pi}{2}} \theta^n \log\sin\theta\, d\theta
\]

There are classical series representations for these integrals, using Fourier series:
\[
\log\sin\theta = -\log 2 - \sum_{k=1}^\infty \frac{\cos 2k\theta}{k}
\]

Thus:
\[
J_n = -\log 2 \int_0^{\frac{\pi}{2}} \theta^n d\theta - \sum_{k=1}^\infty \frac{1}{k} \int_0^{\frac{\pi}{2}} \theta^n \cos 2k\theta\, d\theta
\]

Let’s compute \(\int_0^{\frac{\pi}{2}} \theta^n d\theta\):

- For \( n = 1 \): \(\int_0^{\frac{\pi}{2}} \theta d\theta = \frac{1}{2} \left(\frac{\pi}{2}\right)^2 = \frac{\pi^2}{8} \)
- For \( n = 2 \): \(\int_0^{\frac{\pi}{2}} \theta^2 d\theta = \frac{1}{3} \left(\frac{\pi}{2}\right)^3 = \frac{\pi^3}{24} \)

Let’s compute the general oscillating term:
\[
I_{n,k} = \int_0^{\frac{\pi}{2}} \theta^n \cos 2k\theta\, d\theta
\]

##### For \( J_1 \):

\[
J_1 = -\log 2 \cdot \frac{\pi^2}{8} - \sum_{k=1}^\infty \frac{1}{k} \int_0^{\frac{\pi}{2}} \theta \cos 2k\theta\, d\theta
\]

The standard integral:
\[
\int_0^a x \cos bx\, dx = \left. \frac{1}{b} x \sin bx + \frac{1}{b^2} \cos bx \right|_0^a - \frac{1}{b^2}
\]

Set \(a = \frac{\pi}{2}, b = 2k\):

\[
\int_0^{\frac{\pi}{2}} \theta \cos 2k\theta\, d\theta = \frac{1}{2k} \frac{\pi}{2} \sin(k\pi) + \frac{1}{(2k)^2} \cos(k\pi) - \frac{1}{(2k)^2} \\
= 0 + \frac{1}{4k^2}[(-1)^k - 1]
\]

Thus,
\[
J_1 = -\frac{\pi^2}{8} \log 2 - \sum_{k=1}^\infty \frac{1}{k} \cdot \frac{1}{4k^2}[(-1)^k - 1] \\
= -\frac{\pi^2}{8} \log 2 - \frac{1}{4} \sum_{k=1}^\infty \left(\frac{(-1)^k - 1}{k^3}\right)
\]

Now,
\[
\sum_{k=1}^\infty \left( \frac{(-1)^k - 1}{k^3} \right) = \sum_{k=1}^\infty \frac{(-1)^k}{k^3} - \sum_{k=1}^\infty \frac{1}{k^3}
\]

The first term is the alternating zeta: \(-\eta(3) = -\sum_{k=1}^\infty \frac{(-1)^{k-1}}{k^3} = -\left(1 - \frac{1}{8}\right)\zeta(3) = -\frac{7}{8} \zeta(3)\), but let's write:
\[
\sum_{k=1}^\infty \frac{(-1)^k}{k^3} = -\sum_{k=1}^\infty \frac{(-1)^{k-1}}{k^3} = -\eta(3) = -\left(1 - \frac{1}{2^2}\right)\zeta(3) = -\frac{3}{4}\zeta(3)
\]
But actually for general n:
\[
\sum_{k=1}^\infty \frac{(-1)^{k+1}}{k^n} = \left(1 - \frac{1}{2^{n-1}}\right) \zeta(n)
\]
So
\[
\sum_{k=1}^\infty \frac{(-1)^k}{k^3} = -\left(1 - \frac{1}{2^{2}}\right)\zeta(3) = -\frac{3}{4}\zeta(3)
\]

Also,
\[
\sum_{k=1}^\infty \frac{1}{k^3} = \zeta(3)
\]

So,
\[
\sum_{k=1}^\infty \frac{(-1)^k - 1}{k^3} = -\frac{3}{4}\zeta(3) - \zeta(3) = -\frac{7}{4}\zeta(3)
\]
Thus,
\[
J_1 = -\frac{\pi^2}{8} \log 2 + \frac{7}{16} \zeta(3)
\]

##### For \(J_2\):

Consider

\[
J_2 = -\log 2 \frac{\pi^3}{24} - \sum_{k=1}^\infty \frac{1}{k} \int_0^{\frac{\pi}{2}} \theta^2 \cos 2k\theta\, d\theta
\]

Let's compute \(\int_0^{\frac{\pi}{2}} \theta^2 \cos 2k\theta\, d\theta\):

Use integration by parts. Let \(u = \theta^2\), \(dv = \cos 2k\theta d\theta\),
then \(du = 2\theta d\theta\), \(v = \frac{1}{2k} \sin 2k\theta\):

\[
\int_0^{\frac{\pi}{2}} \theta^2 \cos 2k\theta d\theta = \frac{1}{2k} \left[ \theta^2 \sin 2k\theta \right]_0^{\frac{\pi}{2}} - \frac{1}{2k} \int_0^{\frac{\pi}{2}} 2\theta \sin 2k\theta d\theta
\]

At \(\theta = \frac{\pi}{2}\), \(\sin k\pi = 0\), at \(\theta = 0\), also zero.

\[
= -\frac{1}{k} \int_0^{\frac{\pi}{2}} \theta \sin 2k\theta d\theta
\]

The standard integral:

\[
\int x \sin a x dx = -\frac{x}{a} \cos a x + \frac{1}{a^2} \sin a x
\]

Thus,

\[
\int_0^{\frac{\pi}{2}} \theta \sin 2k\theta d\theta
= \left. -\frac{\theta}{2k} \cos 2k\theta + \frac{1}{(2k)^2} \sin 2k\theta \right|_0^{\frac{\pi}{2}}
\]

At \(\theta=\frac{\pi}{2}\): \(\cos k\pi = (-1)^k\), \(\sin k\pi = 0\)

At \(\theta=0\): \(\cos 0 = 1\), \(\sin 0 = 0\)

So,

\[
= -\frac{\pi}{4k} (-1)^k + 0 - \left(0 - 0\right) = -\frac{\pi}{4k} (-1)^k + \frac{0}{1} = -\frac{\pi}{4k} (-1)^k
\]

Thus

\[
\int_0^{\frac{\pi}{2}} \theta^2 \cos 2k\theta d\theta = -\frac{1}{k} \times \left( -\frac{\pi}{4k} (-1)^k \right) = \frac{\pi}{4 k^2} (-1)^k
\]

So

\[
J_2 = -\frac{\pi^3}{24} \log 2 - \sum_{k=1}^\infty \frac{1}{k} \cdot \frac{\pi}{4 k^2} (-1)^k
= -\frac{\pi^3}{24}\log 2 - \frac{\pi}{4} \sum_{k=1}^\infty \frac{(-1)^k}{k^3}
\]

Recall above:

\[
\sum_{k=1}^\infty \frac{(-1)^k}{k^3} = -\frac{3}{4} \zeta(3)
\]

So,

\[
J_2 = -\frac{\pi^3}{24} \log 2 + \frac{3\pi}{16} \zeta(3)
\]

### Step 4: Substitute back into integral

Recall:
\[
I = -\pi J_1 + 3 J_2
\]

Substitute \(J_1\) and \(J_2\):

\[
I = -\pi\left( -\frac{\pi^2}{8}\log 2 + \frac{7}{16} \zeta(3) \right) + 3\left( -\frac{\pi^3}{24}\log 2 + \frac{3\pi}{16} \zeta(3) \right )
\]
\[
= \frac{\pi^3}{8}\log 2 - \frac{7\pi}{16} \zeta(3) - \frac{\pi^3}{8}\log 2 + \frac{9\pi}{16} \zeta(3)
\]
Note the \(\log 2\) terms cancel.
\[
I = \left( \frac{\pi^3}{8} - \frac{\pi^3}{8} \right) \log 2 + \left( -\frac{7\pi}{16} + \frac{9\pi}{16} \right ) \zeta(3)
= 0 + \frac{2\pi}{16} \zeta(3)
= \frac{\pi}{8} \zeta(3)
\]

### Step 5: Final exact and numerical answers

The exact result is:
\[
\boxed{ \int_0^1 \frac{1}{x} \arccos x \arcsin^2 x \, dx = \frac{\pi}{8} \zeta(3) }
\]

Now for a numerical value:

- \(\pi \approx 3.141592653589793\)
- \(\zeta(3) \approx 1.202056903159594\)

So

\[
I \approx \frac{3.141592653589793}{8} \times 1.202056903159594 \approx 0.4712388980384691
\]

So, to 10 decimal places: \(0.4712388980\)

---

```json
{"answer": "\\frac{\\pi}{8} \\, \\zeta(3)", "numerical_answer": "0.4712388980"}
```