Let's compute the integral
\[
I = \int_0^2 x \arctan\left( \sqrt{x(2-x)} \right) \, dx
\]

**Step 1. Substitution**

Let’s try the substitution \( x = 2 \sin^2 \theta \).  
Then, as \( x \) goes from \( 0 \) to \( 2 \):

- When \( x=0 \), \( \theta=0 \)
- When \( x=2 \), \( \theta = \pi/2 \)

Compute the terms:

\[
x = 2\sin^2\theta
\]
\[
2-x = 2 - 2\sin^2\theta = 2\cos^2\theta
\]
\[
x(2-x) = 2\sin^2\theta \cdot 2\cos^2\theta = 4\sin^2\theta \cos^2\theta = 4\sin^2\theta \cos^2\theta
\]
\[
\sqrt{x(2-x)} = 2\sin\theta \cos\theta = \sin 2\theta
\]
\[
dx = 4\sin\theta \cos\theta d\theta = 2\sin 2\theta d\theta
\]

So, rewrite the integral:

\[
I = \int_{x=0}^{x=2} x \arctan\left( \sqrt{x(2 - x)} \right) dx = \int_{\theta = 0}^{\theta = \pi/2} 2\sin^2\theta \cdot \arctan(\sin 2\theta) \cdot 2\sin 2\theta d\theta
\]
\[
= 4\int_0^{\pi/2} \sin^2 \theta \arctan(\sin 2\theta) \sin 2\theta d\theta
\]

But \(\sin 2\theta = 2\sin\theta\cos\theta\):

\[
I = 4\int_0^{\pi/2} \sin^2\theta \arctan(\sin 2\theta) \cdot \sin 2\theta d\theta
\]

We can write:

\[
I = 4\int_0^{\pi/2} \sin^2\theta \cdot \sin 2\theta \cdot \arctan (\sin 2\theta) d\theta
\]

Let’s write \(\sin^2\theta \sin 2\theta\):

\[
\sin 2\theta = 2\sin\theta\cos\theta
\]
So,
\[
\sin^2\theta \sin 2\theta = 2\sin^3 \theta \cos \theta
\]

Putting all together:

\[
I = 4\int_0^{\pi/2} 2\sin^3 \theta \cos\theta \arctan (\sin 2\theta) d\theta = 8\int_0^{\pi/2} \sin^3\theta \cos\theta \arctan(\sin 2\theta) d\theta
\]

Now, let's make a substitution inside this integral to simplify it.

Let’s try \(u = \sin 2\theta\):

\[
u = \sin 2\theta
\]
\[
du = 2 \cos 2\theta d\theta
\]
But we may find it more useful to write in terms of \(u\), but let's see what \(\sin^3\theta\cos\theta\) becomes in terms of \(u\):

Recall,
- \(\sin^3\theta = \sin\theta \cdot \sin^2\theta = \sin\theta (1-\cos^2\theta)\)
- \(\sin 2\theta = 2\sin\theta\cos\theta \implies \sin\theta\cos\theta = \tfrac{1}{2}\sin 2\theta\)

Let us instead try an integration by parts.

Let
- \(u = \arctan(\sin 2\theta)\)
- \(dv = \sin^3\theta \cos\theta d\theta\)

Then,
- \(du = \frac{2\cos 2\theta}{1+\sin^2 2\theta} d\theta\)
- To compute \(v\), integrate \(dv = \sin^3\theta\cos\theta d\theta\)

Let’s compute \(v = \int \sin^3\theta\cos\theta d\theta\):

Let’s use \(w = \sin\theta\):
Then \(dw = \cos\theta d\theta\)

\[
\sin^3\theta\cos\theta d\theta = w^3 dw
\]
Therefore,
\[
v = \int w^3 dw = \frac{w^4}{4} = \frac{\sin^4\theta}{4}
\]

Now, apply integration by parts:

\[
I = 8 \left(
\left[ \frac{\sin^4\theta}{4}\arctan(\sin 2\theta)\right]_0^{\pi/2}
- \int_0^{\pi/2} \frac{\sin^4\theta}{4}\cdot \frac{2\cos 2\theta}{1 + \sin^2 2\theta}d\theta
\right)
\]

Compute the first term:

At \(\theta = 0\):

- \(\sin^4 0 = 0\)
- So term is 0

At \(\theta = \pi/2\):

- \(\sin^4(\pi/2) = 1\)
- \(\sin 2\theta = \sin \pi = 0\)
- \(\arctan(0) = 0\)
- So term is also 0

Therefore, both boundary terms vanish.

So,

\[
I = -8 \int_{0}^{\pi/2} \frac{\sin^4\theta}{4} \cdot \frac{2\cos 2\theta}{1 + \sin^2 2\theta} d\theta
= -4 \int_0^{\pi/2} \frac{\sin^4\theta \cos 2\theta}{1 + \sin^2 2\theta} d\theta
\]

**Step 2. Simplify the integral**

Let’s expand \(\sin^4 \theta\):

\[
\sin^4 \theta = \left( \sin^2\theta \right)^2 = \left( \frac{1-\cos 2\theta}{2}\right)^2 = \frac{1 - 2\cos 2\theta + \cos^2 2\theta}{4}
\]

So,

\[
I = -4 \int_0^{\pi/2} \frac{1 - 2\cos 2\theta + \cos^2 2\theta}{4} \cdot \frac{\cos 2\theta}{1 + \sin^2 2\theta} d\theta
\]
\[
= -\int_0^{\pi/2} \frac{1 - 2\cos 2\theta + \cos^2 2\theta}{1 + \sin^2 2\theta} \cdot \cos 2\theta d\theta
\]

Let’s split the numerator:

\[
1 - 2\cos 2\theta + \cos^2 2\theta = (\cos 2\theta - 1)^2
\]

Let’s check:
\[
(\cos 2\theta - 1)^2 = \cos^2 2\theta - 2\cos 2\theta + 1
\]
Yes.

So,

\[
I = -\int_0^{\pi/2} \frac{(\cos 2\theta - 1)^2 \cos 2\theta}{1 + \sin^2 2\theta} d\theta
\]

Now, expand \((\cos 2\theta - 1)^2 \cos 2\theta\):

\[
= [\cos^2 2\theta - 2\cos 2\theta + 1] \cos 2\theta = \cos^3 2\theta - 2\cos^2 2\theta + \cos 2\theta
\]

So,

\[
I = -\int_0^{\pi/2} \frac{\cos^3 2\theta - 2\cos^2 2\theta + \cos 2\theta}{1 + \sin^2 2\theta} d\theta
\]

\[
I = -\int_0^{\pi/2} \frac{\cos^3 2\theta}{1 + \sin^2 2\theta} d\theta
+ 2 \int_0^{\pi/2} \frac{\cos^2 2\theta}{1 + \sin^2 2\theta} d\theta
- \int_0^{\pi/2} \frac{\cos 2\theta}{1 + \sin^2 2\theta} d\theta
\]

That is,

\[
I = -A + 2B - C
\]
where
\[
A = \int_0^{\pi/2} \frac{\cos^3 2\theta}{1 + \sin^2 2\theta} d\theta
\]
\[
B = \int_0^{\pi/2} \frac{\cos^2 2\theta}{1 + \sin^2 2\theta} d\theta
\]
\[
C = \int_0^{\pi/2} \frac{\cos 2\theta}{1 + \sin^2 2\theta} d\theta
\]

Let’s try to compute each of these.

**Step 3. Compute C**

Let’s start with \(C\):

\[
C = \int_0^{\pi/2} \frac{\cos 2\theta}{1 + \sin^2 2\theta} d\theta
\]

Let’s let \(u = \sin 2\theta\), \(du = 2\cos2\theta d\theta\), so \(\cos2\theta d\theta = du/2\).

When \(\theta = 0, u = 0\), \(\theta = \pi/2, u = 0\).

So both limits are zero.

Thus
\[
C = \int_0^{\pi/2} \frac{ \cos 2\theta}{1 + \sin^2 2\theta } d\theta = \frac{1}{2} \int_{u=0}^{u=0} \frac{1}{1+u^2} du = 0
\]
(Ah! The integral is zero because the integration range is the same.)

**Step 4. Compute A and B**

Let’s try \(B\):

\[
B = \int_0^{\pi/2} \frac{\cos^2 2\theta}{1 + \sin^2 2\theta} d\theta
\]

Recall: \(\cos^2 2\theta = 1 - \sin^2 2\theta\), so

\[
B = \int_0^{\pi/2} \frac{1 - \sin^2 2\theta}{1 + \sin^2 2\theta} d\theta
= \int_0^{\pi/2} \frac{1}{1 + \sin^2 2\theta} d\theta - \int_0^{\pi/2} \frac{\sin^2 2\theta}{1 + \sin^2 2\theta} d\theta
\]

But \[
\frac{\sin^2 2\theta}{1 + \sin^2 2\theta} = 1 - \frac{1}{1+\sin^2 2\theta}
\]

Therefore,
\[
\int_0^{\pi/2} \frac{\sin^2 2\theta}{1 + \sin^2 2\theta} d\theta = \int_0^{\pi/2} 1 d\theta - \int_0^{\pi/2} \frac{1}{1+\sin^2 2\theta} d\theta = \frac{\pi}{2} - \int_0^{\pi/2} \frac{1}{1 + \sin^2 2\theta} d\theta
\]

Therefore,

\[
B = \int_0^{\pi/2} \frac{1}{1 + \sin^2 2\theta} d\theta - \left( \frac{\pi}{2} - \int_0^{\pi/2} \frac{1}{1 + \sin^2 2\theta} d\theta \right ) = 2 \int_0^{\pi/2} \frac{1}{1 + \sin^2 2\theta} d\theta - \frac{\pi}{2}
\]

Let’s denote \(S = \int_0^{\pi/2} \frac{1}{1 + \sin^2 2\theta} d\theta\), so

\[
B = 2S - \frac{\pi}{2}
\]

Now, for \(A\):

\[
A = \int_0^{\pi/2} \frac{\cos^3 2\theta}{1 + \sin^2 2\theta} d\theta
\]
\[
= \int_0^{\pi/2} \frac{\cos 2\theta \cdot \cos^2 2\theta}{1 + \sin^2 2\theta} d\theta
\]

But \(\cos^2 2\theta = 1 - \sin^2 2\theta\):

\[
A = \int_0^{\pi/2} \frac{\cos 2\theta (1 - \sin^2 2\theta)}{1 + \sin^2 2\theta} d\theta
\]
\[
= \int_0^{\pi/2} \frac{\cos 2\theta}{1 + \sin^2 2\theta} d\theta - \int_0^{\pi/2} \frac{\cos 2\theta \sin^2 2\theta}{1 + \sin^2 2\theta} d\theta
\]

But as we saw earlier, the first term vanishes (since the substitution brings the same limits).

So,
\[
A = - \int_0^{\pi/2} \frac{\cos 2\theta \sin^2 2\theta}{1 + \sin^2 2\theta} d\theta
\]

Let’s write \(\sin^2 2\theta = 1 - \cos^2 2\theta\):

\[
A = - \int_0^{\pi/2} \frac{\cos 2\theta (1 - \cos^2 2\theta)}{1 + \sin^2 2\theta} d\theta
= - \int_0^{\pi/2} \frac{\cos 2\theta}{1 + \sin^2 2\theta} d\theta + \int_0^{\pi/2} \frac{\cos 2\theta \cos^2 2\theta}{1 + \sin^2 2\theta} d\theta
\]

But the first term is again zero, and note that

\[
A = \int_0^{\pi/2} \frac{ \cos^3 2\theta}{1 + \sin^2 2\theta} d\theta
= \int_0^{\pi/2} \frac{ \cos 2\theta \cos^2 2\theta}{1 + \sin^2 2\theta} d\theta
\]

So the integral in the second term is just \(A\) itself.

This seems circular, but let's try to be more concrete.

Alternatively, let's attempt a substitution for
\[
S = \int_0^{\pi/2} \frac{1}{1 + \sin^2 2\theta} d\theta
\]

Let \(u = 2\theta, \, du = 2 d\theta,\, \theta = u/2\) and when \(\theta = 0, u = 0,\) \(\theta = \pi/2, u = \pi\):

\[
S = \int_0^{\pi/2} \frac{1}{1+\sin^2 2\theta} d\theta = \frac{1}{2}\int_0^{\pi} \frac{1}{1+\sin^2 u} du
\]

Now, the definite integral
\[
\int_{0}^{\pi} \frac{du}{1 + \sin^2 u}
\]
can be found using standard tables or advanced techniques.

Let’s further note that
\[
1 + \sin^2 u = 1 + \frac{1 - \cos 2u}{2} = \frac{3}{2} - \frac{1}{2} \cos 2u
\]

Thus,
\[
\int_0^{\pi} \frac{du}{1 + \sin^2 u} = \int_0^{\pi} \frac{2}{3 - \cos 2u} du
\]

Let’s use the identity:

\[
\int_0^\pi \frac{du}{a - \cos u} = \frac{\pi}{\sqrt{a^2 - 1}}, \quad |a| > 1
\]
But here, \(\cos 2u\), so \(du = d(2u)/2\). Let's write \(w = 2u\), \(du = dw/2\), as \(u\) goes from \(0\) to \(\pi\), \(w\) goes from \(0\) to \(2\pi\):

\[
\int_0^{\pi} \frac{2}{3 - \cos 2u} du = 2 \int_0^{\pi} \frac{du}{3 - \cos 2u}
= 2 \cdot \frac{1}{2} \int_0^{2\pi} \frac{dw}{3 - \cos w}
= \int_0^{2\pi} \frac{dw}{3 - \cos w}
\]

From standard tables (see Gradshteyn & Rhyzik 3.723.1):

\[
\int_0^{2\pi} \frac{dw}{a - \cos w} = \frac{2\pi}{\sqrt{a^2 - 1}}, \quad |a| > 1
\]

Here, \(a = 3\):

\[
\int_0^{2\pi} \frac{dw}{3 - \cos w} = \frac{2\pi}{\sqrt{3^2 - 1}} = \frac{2\pi}{\sqrt{8}} = \frac{\pi}{\sqrt{2}}
\]

Therefore,
\[
S = \frac{1}{2} \int_0^\pi \frac{1}{1+\sin^2 u} du = \frac{1}{2} \cdot \frac{\pi}{\sqrt{2}} = \frac{\pi}{2\sqrt{2}}
\]

Now, plugging back in:

\[
B = 2S - \frac{\pi}{2} = \frac{\pi}{\sqrt{2}} - \frac{\pi}{2} = \pi \left( \frac{1}{\sqrt{2}} - \frac{1}{2}\right )
\]

Now, let's recall our expression for \(I\):

Since \(C = 0\), and

\[
I = -A + 2B
\]

Now, let's tackle \(A\):

Recall, from earlier,
\[
A = \int_0^{\pi/2} \frac{\cos^3 2\theta}{1+\sin^2 2\theta} d\theta
\]

Let’s express \(\cos^3 2\theta\) as \(\cos 2\theta (1 - \sin^2 2\theta) \):

\[
\cos^3 2\theta = \cos 2\theta (1 - \sin^2 2\theta ) = \cos 2\theta - \cos 2\theta \sin^2 2\theta
\]

Thus,
\[
A = \int_0^{\pi/2} \frac{\cos 2\theta}{1+\sin^2 2\theta} d\theta - \int_0^{\pi/2} \frac{\cos 2\theta \sin^2 2\theta}{1+\sin^2 2\theta} d\theta
\]

But as before, the first term is zero, as shown in Step 3.

So
\[
A = - \int_0^{\pi/2} \frac{\cos 2\theta \sin^2 2\theta}{1+\sin^2 2\theta} d\theta
\]

But
\[
\frac{\cos 2\theta \sin^2 2\theta}{1+\sin^2 2\theta} = \cos 2\theta - \frac{\cos 2\theta}{1+\sin^2 2\theta}
\]

Therefore,
\[
A = - \int_0^{\pi/2} \cos 2\theta d\theta + \int_0^{\pi/2} \frac{ \cos 2\theta}{1+\sin^2 2\theta} d\theta
\]

But again, the second term is zero; only the first term remains,
\[
A = - \int_0^{\pi/2} \cos 2\theta d\theta
\]
\[
= - \left[ \frac{\sin 2\theta}{2} \right]_0^{\pi/2}
= - \left( \frac{\sin \pi}{2} - \frac{\sin 0}{2} \right ) = 0
\]

Therefore, \(A = 0\).

Thus,
\[
I = 2 B = 2 \pi \left( \frac{1}{\sqrt{2}} - \frac{1}{2}\right )
= \pi \left( \frac{2}{\sqrt{2}} - 1 \right )
= \pi ( \sqrt{2} - 1 )
\]

**Final Answer**
\[
\boxed{
I = \int_0^2 x \arctan\left( \sqrt{x(2-x)} \right) dx = \pi (\sqrt{2} - 1)
}
\]

**Numerical Approximation:**
\[
\pi (\sqrt{2} - 1) \approx 3.1415926535 \times (1.4142135624 - 1) \approx 3.1415926535 \times 0.4142135624 \approx 1.3012902845
\]

**JSON Output**
```json
{"answer": "\\pi(\\sqrt{2} - 1)", "numerical_answer": "1.3012902845"}
```