We start with the integral

  I = ∫₀∞ x^(2-1) e^(–1.0·x²) H₂(1.0·x) dx.

Since 2 – 1 = 1, this simplifies to

  I = ∫₀∞ x e^(–x²) H₂(x) dx.

Using the definition of the (physicists’) Hermite polynomials, we have

  H₂(x) = 4x² – 2.

Thus the integral becomes

  I = ∫₀∞ x e^(–x²) (4x² – 2) dx = 4 ∫₀∞ x³ e^(–x²) dx – 2 ∫₀∞ x e^(–x²) dx.

We now evaluate each term separately using the formula

  ∫₀∞ xⁿ e^(–x²) dx = ½ · Γ((n + 1)/2).

For the first integral with n = 3:
  ∫₀∞ x³ e^(–x²) dx = ½ · Γ((3 + 1)/2) = ½ · Γ(2) = ½ · 1! = ½.

For the second integral with n = 1:
  ∫₀∞ x e^(–x²) dx = ½ · Γ((1 + 1)/2) = ½ · Γ(1) = ½ · 1 = ½.

Substituting these back, we get

  I = 4·(½) – 2·(½) = 2 – 1 = 1.

Thus, the exact answer is 1. Its numerical approximation is 1.0000000000.

{"answer": "$1$", "numerical_answer": "1.0000000000"}