We will show that
  I = ∫₀¹ [sin(log x) – log x]⁄[log² x] dx = –2 ln(1+√2).

Below are the steps.

Step 1. Change of variable

Let
  u = log x   so that x = eᵘ   and dx = eᵘ du.
When x goes from 0 to 1, u runs from –∞ to 0. In u–terms the integral becomes

  I = ∫₋∞⁰ [sin u – u]⁄u² · eᵘ du.

Next, substitute
  t = –u   so that u = –t   and du = –dt.
The limits now become: when u = –∞, t = ∞ and when u = 0, t = 0.
Also note that sin u = sin(–t) = – sin t and u² = t². Thus

  I = ∫ₜ=∞⁰ [– sin t + t]⁄t² · e^(–t) (–dt)
    = ∫₀∞ [t – sin t]⁄t² · e^(–t) dt.           (1)

Step 2. A parameter–differentiation approach

In order to “tame” the integrals we introduce a parameter. Define for real a

  J(a) = ∫₀¹ { sin(a log x) – a log x }⁄[log² x] dx.
Note that for a = 1 we recover the desired I: I = J(1).

Differentiate under the integral sign with respect to a. Since

  ∂/∂a sin(a log x) = cos(a log x) · log x  and ∂/∂a (– a log x) = – log x,
we have

  J′(a) = ∫₀¹ { cos(a log x)·log x – log x }⁄[log² x] dx
     = ∫₀¹ [cos(a log x) – 1]⁄[log x] dx.

Now change variable again: set y = log x so that x = eʸ and dx = eʸ dy, with y going from –∞ to 0. Then

  J′(a) = ∫₋∞⁰ [cos(a y) – 1]⁄y · eʸ dy.
Next substitute u = – y. Then y = –u, dy = –du, and the limits become u: 0 → ∞. Also cos(a y) = cos(–a u) = cos(a u). Hence

  J′(a) = ∫₀∞ [cos(a u) – 1]⁄u · e^(–u) du.      (2)

There is a standard formula (see, e.g., Gradstein‐Ryzhik)
  ∫₀∞ [1 – cos(p u)] e^(–q u) du⁄u = ln[(q + √(q² + p²))/p]
for p > 0 and q > 0. (The subtraction “1 – cos(p u)” makes the u–integral convergent at 0.) Applying this with p = a and q = 1 gives

  ∫₀∞ [1 – cos(a u)] e^(–u) du⁄u = ln[(1+√(1+a²))/a].

Since our integrand in (2) is cos(a u) – 1, we obtain
  J′(a) = – ln[(1+√(1+a²))/a].      (3)

Step 3. Recovering J(a)

We know J(0) = 0 (this is immediate, since for a = 0 the numerator in the definition of J(a) vanishes). Hence,
  J(a) = ∫₀ᵃ J′(t) dt = – ∫₀ᵃ ln[(1+√(1+t²))/t] dt.
In particular,
  I = J(1) = – ∫₀¹ ln[(1+√(1+t²))/t] dt.      (4)

Step 4. Evaluation of the remaining one–dimensional integral

To evaluate
  L = ∫₀¹ ln[(1+√(1+t²))/t] dt,
make the substitution
  t = sinh θ,   so that dt = cosh θ dθ   and √(1+t²) = cosh θ.
When t ranges from 0 to 1, θ ranges from 0 to asinh(1) = ln(1+√2). Then
  L = ∫₀^(ln(1+√2)) ln[(1+cosh θ)/(sinh θ)] cosh θ dθ.
A well–known hyperbolic identity shows that
  (1+cosh θ)/(sinh θ) = coth (θ/2).
Thus,
  L = ∫₀^(ln(1+√2)) cosh θ · ln[coth(θ/2)] dθ.
Now integrate by parts. Let
  u = ln[coth(θ/2)]   and dv = cosh θ dθ.
Then
  du = – (1/sinh θ)dθ   (since d/dθ ln[coth(θ/2)] = –1/sinh θ)
and
  v = sinh θ.
Thus,
  L = [sinh θ · ln(coth(θ/2))]₀^(ln(1+√2)) – ∫₀^(ln(1+√2)) sinh θ · (–1/sinh θ) dθ
    = [sinh θ · ln(coth(θ/2))]₀^(ln(1+√2)) + ∫₀^(ln(1+√2)) dθ.
At θ = 0 the product vanishes (one may check the limit); so
  L = sinh(asinh 1) · ln(coth(asinh 1⁄2)) + asinh 1.
But sinh(asinh 1) = 1 and asinh 1 = ln(1+√2). Also, one may show that
  coth[(1/2) ln(1+√2)] = 1+√2.
Thus,
  L = ln(1+√2) + ln(1+√2) = 2 ln(1+√2).

Returning to (4) we now have
  I = – L = –2 ln(1+√2).

Step 5. Numerical approximation

We compute 1+√2. Since √2 ≈ 1.4142135624, we have 1+√2 ≈ 2.4142135624. Then,
  I ≈ –2 · ln(2.4142135624) ≈ –2 · 0.881373 (since ln(2.4142135624) ≈ 0.881373)
    ≈ –1.7627461393.

Thus, the exact answer is –2 ln(1+√2) and the numerical approximation (to 10 decimal places) is –1.7627461393.

{"answer": "-2\\ln\\left(1+\\sqrt{2}\\right)", "numerical_answer": "-1.7627461393"}