Let's define the integral:
\[
I = \int_0^1 \left( (1-x^{25})^{1/20} - (1-x^{20})^{1/25} \right) dx
\]

---

### Step 1: Tackle Each Term Separately

#### First Term: \(\int_0^1 (1-x^{25})^{1/20} dx\)

Let \( u = x^{25} \implies x = u^{1/25} \implies dx = \frac{1}{25} u^{-24/25} du \). When \(x=0,\, u=0\); when \(x=1,\, u=1\):

\[
\int_0^1 (1-x^{25})^{1/20} dx = \int_{u=0}^{u=1} (1-u)^{1/20} \cdot \frac{1}{25} u^{-24/25} du
\]
\[
= \frac{1}{25} \int_0^1 (1-u)^{1/20} u^{-24/25} du
\]

#### Second Term: \(\int_0^1 (1-x^{20})^{1/25} dx\)

Let \( v = x^{20} \implies x = v^{1/20} \implies dx = \frac{1}{20} v^{-19/20} dv \):

\[
\int_0^1 (1-x^{20})^{1/25} dx = \int_{v=0}^{v=1} (1-v)^{1/25} \cdot \frac{1}{20} v^{-19/20} dv
\]
\[
= \frac{1}{20} \int_0^1 (1-v)^{1/25} v^{-19/20} dv
\]

---

### Step 2: Express in Terms of Beta and Gamma Functions

Recall:
\[
B(p,q) = \int_0^1 t^{p-1}(1-t)^{q-1} dt = \frac{\Gamma(p)\Gamma(q)}{\Gamma(p+q)}
\]

##### First Integral:
\[
\frac{1}{25} \int_0^1 u^{-24/25} (1-u)^{1/20} du = \frac{1}{25} \cdot B\left(1-\frac{24}{25},\, 1+\frac{1}{20}\right)
\]
\[
= \frac{1}{25} \cdot B\left(\frac{1}{25},\, \frac{21}{20}\right)
\]
\[
= \frac{1}{25} \cdot \frac{\Gamma(\frac{1}{25}) \Gamma(\frac{21}{20})}{\Gamma(\frac{1}{25}+\frac{21}{20})}
\]

##### Second Integral:
\[
\frac{1}{20} \int_0^1 v^{-19/20} (1-v)^{1/25} dv = \frac{1}{20} \cdot B\left(1-\frac{19}{20},\, 1+\frac{1}{25}\right)
\]
\[
= \frac{1}{20} B\left(\frac{1}{20},\, \frac{26}{25}\right)
\]
\[
= \frac{1}{20} \cdot \frac{\Gamma(\frac{1}{20}) \Gamma(\frac{26}{25})}{\Gamma(\frac{1}{20}+\frac{26}{25})}
\]

---

### Step 3: The Final Expression

So,
\[
I = \boxed{
\frac{1}{25} \cdot \frac{\Gamma(\frac{1}{25}) \Gamma(\frac{21}{20})}{\Gamma(\frac{1}{25}+\frac{21}{20})}
-
\frac{1}{20} \cdot \frac{\Gamma(\frac{1}{20}) \Gamma(\frac{26}{25})}{\Gamma(\frac{1}{20}+\frac{26}{25})}
}
\]

---

### Step 4: Numerical Approximation

Let's compute each term using the values of the Gamma function:

Compute each argument:
- \(\frac{1}{25} = 0.04\)
- \(\frac{21}{20} = 1.05\)
- \(\frac{1}{25} + \frac{21}{20} = 0.04 + 1.05 = 1.09\)

- \(\frac{1}{20} = 0.05\)
- \(\frac{26}{25} = 1.04\)
- \(\frac{1}{20} + \frac{26}{25} = 0.05 + 1.04 = 1.09\)

Calculate with these values:

- \(\Gamma(0.04) \approx 24.53252907\)
- \(\Gamma(1.05) \approx 0.951832\)
- \(\Gamma(1.09) \approx 0.91710912\)

- \(\Gamma(0.05) \approx 19.48727054\)
- \(\Gamma(1.04) \approx 0.967051\)
- \(\Gamma(1.09) \approx 0.91710912\)

Now calculate:

First term:
\[
A = \frac{1}{25} \cdot \frac{24.53252907 \times 0.951832}{0.91710912} \\
= \frac{1}{25} \cdot \frac{23.33891084}{0.91710912} \\
= \frac{1}{25} \cdot 25.44848532 \\
= 1.017939413
\]

Second term:
\[
B = \frac{1}{20} \cdot \frac{19.48727054 \times 0.967051}{0.91710912} \\
= \frac{1}{20} \cdot \frac{18.85708542}{0.91710912} \\
= \frac{1}{20} \cdot 20.56110997 \\
= 1.028055498
\]

So the answer is:
\[
I \approx 1.017939413 - 1.028055498 = -0.010116085
\]

---

### Step 5: Format Answer

```json
{"answer": "\\frac{1}{25} \\frac{\\Gamma\\left(\\frac{1}{25}\\right) \\Gamma\\left(\\frac{21}{20}\\right)}{\\Gamma\\left(\\frac{1}{25}+\\frac{21}{20}\\right)} - \\frac{1}{20} \\frac{\\Gamma\\left(\\frac{1}{20}\\right) \\Gamma\\left(\\frac{26}{25}\\right)}{\\Gamma\\left(\\frac{1}{20}+\\frac{26}{25}\\right)}", "numerical_answer": "-0.0101160850"}
```