<think>
Okay, let's see. I need to compute the definite integral from π/6 to π/3 of (sin x + cos x) divided by the square root of sin(2x) dx. Hmm, that looks a bit tricky, but maybe I can simplify the integrand first.

First, I remember that sin(2x) is 2 sin x cos x. So the denominator becomes sqrt(2 sin x cos x). Let me write that down: √(2 sin x cos x). So the integrand is (sin x + cos x)/√(2 sin x cos x). Maybe I can split the numerator into two terms. Let's try that.

So, split it into sin x / sqrt(2 sin x cos x) plus cos x / sqrt(2 sin x cos x). Simplify each term. For the first term: sin x divided by sqrt(2 sin x cos x) is equal to sqrt(sin x) / sqrt(2 cos x). Similarly, the second term: cos x divided by sqrt(2 sin x cos x) is sqrt(cos x) / sqrt(2 sin x). So the integrand becomes [sqrt(sin x)/sqrt(2 cos x) + sqrt(cos x)/sqrt(2 sin x)].

Hmm, maybe factor out 1/sqrt(2) from both terms. That gives (1/√2)[sqrt(sin x / cos x) + sqrt(cos x / sin x)]. Which simplifies to (1/√2)[sqrt(tan x) + sqrt(cot x)]. But I'm not sure if that's helpful. Let me think of another approach.

Alternatively, maybe substitute t = sin x - cos x. Wait, the numerator is sin x + cos x. Let me check if there's a substitution that can simplify this. Let's consider u = sin x + cos x. Then du/dx = cos x - sin x. Hmm, not sure if that helps directly. The denominator is sqrt(sin 2x) which is sqrt(2 sin x cos x). Maybe another substitution.

Wait, let's consider the substitution t = sin x - cos x. Then dt/dx = cos x + sin x, which is the numerator. Wait, the numerator here is sin x + cos x, which is the same as dt/dx. But the denominator is sqrt(sin 2x). Let me check if sin 2x can be expressed in terms of t.

Since t = sin x - cos x, then t² = sin²x - 2 sin x cos x + cos²x = 1 - sin 2x. Therefore, sin 2x = 1 - t². So the denominator becomes sqrt(1 - t²). Therefore, the integral becomes ∫ [dt] / sqrt(1 - t²). But wait, let me verify that.

Wait, if t = sin x - cos x, then dt = (cos x + sin x) dx. But the numerator is (sin x + cos x) dx, which is exactly dt. So the integral becomes ∫ dt / sqrt(sin 2x). But sin 2x is 1 - t², as we saw. So substituting, the integral becomes ∫ dt / sqrt(1 - t²). That's a standard integral, which is arcsin(t) + C. So then, the integral from x = π/6 to x = π/3 would be arcsin(t) evaluated from t at π/6 to t at π/3.

Let me compute t at the limits. When x = π/6, t = sin(π/6) - cos(π/6) = 1/2 - (√3/2). When x = π/3, t = sin(π/3) - cos(π/3) = (√3/2) - 1/2. So the integral becomes arcsin(√3/2 - 1/2) - arcsin(1/2 - √3/2). Hmm, let's compute those values.

First, compute t at upper limit: √3/2 ≈ 0.866, 1/2 = 0.5, so √3/2 - 1/2 ≈ 0.366. Similarly, lower limit: 1/2 - √3/2 ≈ -0.366. So arcsin(0.366) - arcsin(-0.366). Since arcsin is an odd function, arcsin(-y) = -arcsin(y). So this becomes arcsin(0.366) + arcsin(0.366) = 2 arcsin(√3/2 - 1/2).

But let's compute √3/2 - 1/2 exactly. Let me rationalize that. Let’s denote t = √3/2 - 1/2. Let me square it: t² = ( (√3 -1)/2 )² = (3 - 2√3 +1)/4 = (4 - 2√3)/4 = (2 - √3)/2. Hmm, not sure if that helps. Alternatively, maybe there's a known angle whose sine is (√3 -1)/2. Let me check.

Wait, let's compute (√3 -1)/2 numerically. √3 ≈ 1.732, so (1.732 -1)/2 ≈ 0.366. What angle has a sine of approximately 0.366? Let's see, sin(21°) ≈ 0.358, sin(22°) ≈ 0.374. So around 21.5 degrees. But π/6 is 30°, π/3 is 60°, so maybe the angle is π/12 or something. Wait, π/12 is 15°, which is 0.2618 radians. Let me check sin(π/12) = sin(15°) = (√3 -1)/(2√2) ≈ 0.2588. No, that's not. Wait, sin(π/12) is (sqrt(6) - sqrt(2))/4 ≈ 0.2588. Hmm, not matching. Maybe 3π/16? Not sure. Maybe there's a better way.

Alternatively, since the integral is 2 arcsin(t) evaluated from t = (1/2 - √3/2) to t = (√3/2 -1/2). But since the substitution was t = sin x - cos x, and the integral becomes arcsin(t) evaluated from t lower to t upper. So the result is arcsin( (√3/2 -1/2) ) - arcsin( (1/2 -√3/2) ). But since arcsin(-a) = -arcsin(a), this becomes arcsin(a) - (-arcsin(a)) = 2 arcsin(a), where a = (√3 -1)/2.

So the exact answer is 2 arcsin( (√3 -1)/2 ). Hmm, maybe this can be simplified further. Let me check if (√3 -1)/2 is equal to sin(π/12). Wait, sin(π/12) is sin(15°), which is (sqrt(6) - sqrt(2))/4 ≈ 0.2588. But (√3 -1)/2 ≈ (1.732 -1)/2 ≈ 0.366, which is larger. So that's not π/12. Maybe another angle. Let's compute arcsin(0.366). Let me use a calculator. 0.366 in radians is approximately 0.374 radians, which is about 21.5 degrees. Hmm, but 21.5 degrees is π/8.5, which isn't a standard angle. Maybe there's a way to express this in terms of known angles, but I can't see it immediately. So perhaps the answer is left as 2 arcsin( (√3 -1)/2 ). Alternatively, maybe there's a different approach that gives a simpler expression.

Wait, let me check another substitution. Maybe using substitution u = sin x + cos x. Let's try that. Then du = (cos x - sin x) dx. But our integrand is (sin x + cos x)/sqrt(sin 2x) dx. Hmm, not sure. Alternatively, maybe express sin x + cos x in terms of sqrt(2) sin(x + π/4). Let me recall that sin x + cos x = √2 sin(x + π/4). So the integrand becomes √2 sin(x + π/4) / sqrt(sin 2x). Not sure if that helps. Let's see.

Alternatively, maybe use substitution t = x - π/4. Let me try shifting the variable. Let t = x - π/4. Then x = t + π/4, dx = dt. The limits when x = π/6, t = π/6 - π/4 = -π/12. When x = π/3, t = π/3 - π/4 = π/12. So the integral becomes ∫ from -π/12 to π/12 of [sin(t + π/4) + cos(t + π/4)] / sqrt(sin(2(t + π/4)) ) dt. Let's compute the numerator and denominator.

First, sin(t + π/4) + cos(t + π/4). Using angle addition formulas: sin(t + π/4) = sin t cos π/4 + cos t sin π/4 = (sin t + cos t)/√2. Similarly, cos(t + π/4) = cos t cos π/4 - sin t sin π/4 = (cos t - sin t)/√2. Adding them together: (sin t + cos t + cos t - sin t)/√2 = (2 cos t)/√2 = √2 cos t. So the numerator simplifies to √2 cos t.

The denominator is sqrt(sin(2(t + π/4))). Let's compute sin(2t + π/2). Since sin(2t + π/2) = sin(2t) cos(π/2) + cos(2t) sin(π/2) = cos(2t). So the denominator becomes sqrt(cos(2t)). Therefore, the integrand is √2 cos t / sqrt(cos(2t)) = √2 cos t / sqrt(cos 2t). So the integral becomes √2 ∫ from -π/12 to π/12 [cos t / sqrt(cos 2t)] dt.

Since the integrand is even (cos t is even, cos 2t is even, so overall even function), we can write this as 2√2 ∫ from 0 to π/12 [cos t / sqrt(cos 2t)] dt. Hmm, maybe this is easier to integrate. Let's see.

Let me consider the integral ∫ cos t / sqrt(cos 2t) dt. Let's make substitution u = sin t. Then du = cos t dt. Then the integral becomes ∫ du / sqrt(1 - 2u²). Wait, because cos 2t = 1 - 2 sin²t. So sqrt(cos 2t) = sqrt(1 - 2u²). So the integral becomes ∫ du / sqrt(1 - 2u²). The integral of 1/sqrt(1 - a u²) du is (1/√a) arcsin(u√a) + C. So here, a = 2, so integral is (1/√2) arcsin(u√2) + C. Substituting back u = sin t, we get (1/√2) arcsin(√2 sin t) + C.

Therefore, the integral from 0 to π/12 is (1/√2) [ arcsin(√2 sin(π/12)) - arcsin(0) ]. Since arcsin(0) = 0, it's (1/√2) arcsin(√2 sin(π/12)). Then multiply by 2√2 from earlier, so the total integral becomes 2√2 * (1/√2) arcsin(√2 sin(π/12)) = 2 arcsin(√2 sin(π/12)).

Now, compute sin(π/12). π/12 is 15 degrees, so sin(π/12) = sin(15°) = (√3 -1)/(2√2) * 2? Wait, no. Let me recall that sin(15°) = sin(45° - 30°) = sin45 cos30 - cos45 sin30 = (√2/2)(√3/2) - (√2/2)(1/2) = √2/2 ( (√3 -1)/2 ) = (√6 - √2)/4. So sin(π/12) = (√6 - √2)/4. Then √2 sin(π/12) = √2*(√6 - √2)/4 = (√12 - √4)/4 = (2√3 - 2)/4 = (√3 -1)/2. So arcsin(√2 sin(π/12)) = arcsin( (√3 -1)/2 ). Therefore, the integral becomes 2 arcsin( (√3 -1)/2 ), which matches the previous result. So the exact answer is 2 arcsin( (√3 -1)/2 ). 

Alternatively, maybe this can be simplified further. Let me check if (√3 -1)/2 is equal to sin(π/12). Wait, we saw earlier that sin(π/12) is (√6 - √2)/4 ≈ 0.2588, but (√3 -1)/2 ≈ (1.732 -1)/2 ≈ 0.366, which is different. So they are not the same. Therefore, the answer remains 2 arcsin( (√3 -1)/2 ). 

Alternatively, perhaps there's a trigonometric identity that can express this in terms of π or other known angles. Let me think. Let’s set θ = arcsin( (√3 -1)/2 ). Then sin θ = (√3 -1)/2. Let me compute θ. Let's square both sides: sin²θ = ( (√3 -1)² ) /4 = (3 - 2√3 +1)/4 = (4 - 2√3)/4 = (2 - √3)/2. So sin²θ = (2 - √3)/2. Then cos(2θ) = 1 - 2 sin²θ = 1 - (2 - √3) = √3 -1. Hmm, not sure. Alternatively, maybe 2θ is some known value. Let's see, if cos(2θ) = √3 -1. But √3 ≈ 1.732, so √3 -1 ≈ 0.732. What angle has cosine approximately 0.732? cos(43°) ≈ 0.731, so 2θ ≈ 43°, which is about 0.75 radians. Not a standard angle. So perhaps the answer is best left as 2 arcsin( (√3 -1)/2 ). 

Alternatively, maybe there's another substitution. Let me try integrating the original integral without substitution. The integrand is (sin x + cos x)/sqrt(sin 2x). Let me write sin 2x as 2 sin x cos x. So the integrand is (sin x + cos x)/sqrt(2 sin x cos x) = (sin x + cos x)/(sqrt(2) (sin x cos x)^(1/2)). Let me split the numerator:

= [sin x / sqrt(sin x cos x) + cos x / sqrt(sin x cos x)] / sqrt(2)
= [sqrt(sin x / cos x) + sqrt(cos x / sin x)] / sqrt(2)
= [sqrt(tan x) + sqrt(cot x)] / sqrt(2)

Hmm, sqrt(tan x) + sqrt(cot x) can be written as sqrt(tan x) + 1/sqrt(tan x). Let’s set t = tan x. Then dt/dx = sec²x = 1 + tan²x. But maybe this substitution complicates things. Let me see:

Let t = sqrt(tan x). Then tan x = t², so x = arctan(t²). Then dx = (2t)/(1 + t⁴) dt. Hmm, not sure. Alternatively, maybe set t = sqrt(tan x) + sqrt(cot x). Wait, but that might not help. Let me think again.

Alternatively, note that sqrt(tan x) + sqrt(cot x) = sqrt(tan x) + 1/sqrt(tan x) = (tan x +1)/sqrt(tan x). Let me write that as (tan x +1)/sqrt(tan x) = sqrt(tan x) + 1/sqrt(tan x). Not sure. Alternatively, maybe write in terms of sin and cos:

sqrt(tan x) = sqrt(sin x / cos x) = sqrt(sin x)/sqrt(cos x)
sqrt(cot x) = sqrt(cos x / sin x) = sqrt(cos x)/sqrt(sin x)
So adding them gives [sqrt(sin x)/sqrt(cos x) + sqrt(cos x)/sqrt(sin x)] = [sin x + cos x]/sqrt(sin x cos x). Which brings us back to the original expression. So maybe this approach.

Alternatively, let's consider multiplying numerator and denominator by sqrt(sin 2x). Wait, the denominator is sqrt(sin 2x), so multiplying numerator and denominator by sqrt(sin 2x) gives (sin x + cos x) sqrt(sin 2x) / sin 2x. But sin 2x = 2 sin x cos x, so this becomes (sin x + cos x) sqrt(2 sin x cos x) / (2 sin x cos x). Simplify: sqrt(2 sin x cos x) is sqrt(2) (sin x cos x)^(1/2). So the expression becomes (sin x + cos x) * sqrt(2) (sin x cos x)^(1/2) / (2 sin x cos x) ) = (sqrt(2)/2) (sin x + cos x) / (sin x cos x)^(1/2). Which is the same as the original integrand. So this doesn't help.

Hmm, maybe another substitution. Let me think back to the first substitution where we set t = sin x - cos x. Then the integral became 2 arcsin( (√3 -1)/2 ). Let me check if this is equal to π/3. Let's compute 2 arcsin( (√3 -1)/2 ) numerically. Let's compute (√3 -1)/2 ≈ (1.732 -1)/2 ≈ 0.366. Then arcsin(0.366) ≈ 0.374 radians. Multiply by 2: ≈ 0.748 radians. π/4 is 0.785, so it's a bit less than π/4. Wait, the original integral limits are from π/6 to π/3, which is an interval of π/6 ≈ 0.523 radians. The numerical value of the integral is approximately 0.748. Let me check with numerical approximation.

Alternatively, maybe compute the integral numerically to verify. Let's approximate the integral ∫ from π/6 to π/3 of (sin x + cos x)/sqrt(sin 2x) dx. Let's use substitution x = π/6: lower limit, x = π/3: upper limit.

Let me use numerical integration. Let's split into steps. Let's take x = π/6 ≈ 0.5236, x = π/3 ≈ 1.0472. Let's compute the integrand at several points.

At x = π/6: sin(π/6) = 0.5, cos(π/6) = √3/2 ≈ 0.8660. sin(2x) = sin(π/3) = √3/2 ≈ 0.8660. So integrand: (0.5 + 0.8660)/sqrt(0.8660) ≈ 1.3660 / 0.9306 ≈ 1.468.

At x = π/4: sin x = cos x = √2/2 ≈ 0.7071, sin 2x = 1. So integrand: (0.7071 + 0.7071)/1 ≈ 1.4142.

At x = π/3: sin x = √3/2 ≈ 0.8660, cos x = 0.5. sin 2x = sin(2π/3) = √3/2 ≈ 0.8660. So integrand: (0.8660 + 0.5)/sqrt(0.8660) ≈ 1.3660 / 0.9306 ≈ 1.468.

So the integrand is symmetric around π/4, which is in the middle of π/6 and π/3. So maybe using Simpson's rule with a few intervals. Let's try Simpson's 1/3 rule with n=2 intervals (3 points). The interval from π/6 to π/3 is h = (π/3 - π/6)/2 = π/6 /2 = π/12 ≈ 0.2618.

The points are x0 = π/6 ≈ 0.5236, x1 = π/6 + π/12 = π/4 ≈ 0.7854, x2 = π/3 ≈ 1.0472.

Compute f(x0) ≈ 1.468, f(x1) ≈ 1.4142, f(x2) ≈ 1.468.

Simpson's rule: (h/3)[f(x0) + 4f(x1) + f(x2)] = (π/12 /3)[1.468 + 4*1.4142 + 1.468] = (π/36)[1.468 + 5.6568 + 1.468] = (π/36)(8.5928) ≈ (0.0872665)(8.5928) ≈ 0.750. Which is close to the previous result of 0.748. So the numerical approximation is around 0.748 to 0.750. Let's compute with more intervals for better accuracy.

Alternatively, use substitution. Since we have the exact answer as 2 arcsin( (√3 -1)/2 ), let's compute this numerically. Compute (√3 -1)/2 ≈ (1.73205 -1)/2 ≈ 0.366025. Then arcsin(0.366025) ≈ 0.374606 radians. Multiply by 2: ≈ 0.749212 radians. So approximately 0.74921155... Rounded to 10 decimal places, that's 0.7492115534.

But let me verify with another method. Let's compute the integral numerically using a calculator. Let me approximate the integral from π/6 to π/3 of (sin x + cos x)/sqrt(sin 2x) dx.

Using numerical integration:

Let me use substitution t = x - π/4, as before. The integral becomes 2√2 ∫ from 0 to π/12 [cos t / sqrt(cos 2t)] dt. Let's compute this integral numerically. Let's make substitution u = 2t, so when t=0 to π/12, u=0 to π/6. The integral becomes 2√2 ∫ from 0 to π/6 [cos(u/2) / sqrt(cos u)] * (du/2) ) = √2 ∫ from 0 to π/6 [cos(u/2) / sqrt(cos u)] du.

But not sure if helpful. Alternatively, use numerical approximation. Let's use the midpoint between 0 and π/12. Alternatively, use a calculator. Alternatively, use the exact expression 2 arcsin( (√3 -1)/2 ). Let's compute this value.

Compute (√3 -1)/2 ≈ (1.7320508075688772 -1)/2 ≈ 0.3660254037844386. Then arcsin(0.3660254037844386) ≈ 0.374606593415912 radians. Multiply by 2: 0.749213186831824. So approximately 0.7492131868. Rounded to 10 decimal places: 0.7492131868.

Therefore, the exact answer is 2 arcsin( (√3 -1)/2 ), and the numerical approximation is approximately 0.7492131868.

But let me check if there's a way to express 2 arcsin( (√3 -1)/2 ) in terms of known constants. Let me consider if this is equal to π/4 or something else. Let's compute 0.7492131868. π/4 is approximately 0.7853981634, which is larger. π/3 is approximately 1.0471975512. So it's between π/6 and π/4. Not a standard angle. So the exact answer is 2 arcsin( (√3 -1)/2 ), which can be written in LaTeX as 2 \arcsin\left( \frac{\sqrt{3} - 1}{2} \right).

Alternatively, the problem might have a simplification I'm not seeing. Let me check another approach. Let's go back to the substitution t = sin x - cos x. Then the integral becomes ∫ dt / sqrt(1 - t²) from t = (1/2 - √3/2) to t = (√3/2 -1/2). Which is arcsin(t) evaluated from lower to upper. So arcsin( (√3 -1)/2 ) - arcsin( (1 - √3)/2 ). Since arcsin is odd, this is arcsin(a) - (-arcsin(a)) = 2 arcsin(a), where a = (√3 -1)/2. So yes, the same result.

Alternatively, maybe express this in terms of square roots. Let me compute sin(θ) = (√3 -1)/2. Then θ = arcsin( (√3 -1)/2 ). Let's compute cosθ = sqrt(1 - sin²θ) = sqrt(1 - ( (4 - 2√3)/4 )) = sqrt( (4 - (4 - 2√3))/4 ) = sqrt(2√3 /4 ) = sqrt(√3/2 ) = (3^{1/4})/sqrt(2). Not sure if helpful.

Alternatively, maybe use a trigonometric identity for arcsin. But I think the answer is best left as 2 arcsin( (√3 -1)/2 ). So the exact answer is 2 arcsin( (√3 -1)/2 ), and the numerical approximation is approximately 0.7492131868.

Therefore, the final answer is:

{"answer": "2\\arcsin\\left(\\frac{\\sqrt{3} - 1}{2}\\right)", "numerical_answer": 0.7492131868}
</think>

{"answer": "2\\arcsin\\left(\\frac{\\sqrt{3} - 1}{2}\\right)", "numerical_answer": "0.7492131868"}