<think>
Okay, let's tackle this integral step by step. The problem is to compute the definite integral from 0 to 1 of (x³ + x + 1)/(3x² - 3x + 4) dx. Hmm, integrating a rational function. I remember that when the degree of the numerator is higher than the denominator, we should start by performing polynomial long division. Let me check the degrees here. The numerator is a cubic (degree 3) and the denominator is quadratic (degree 2). So yes, we need to divide first.

First, let's perform the division of x³ + x + 1 by 3x² - 3x + 4. To do this, I'll divide the leading terms: x³ divided by 3x² gives (1/3)x. Multiply the denominator by (1/3)x: (1/3)x*(3x² - 3x + 4) = x³ - x² + (4/3)x. Subtract this from the original numerator:

(x³ + x + 1) - (x³ - x² + (4/3)x) = 0 + x² - (1/3)x + 1.

So the remainder is x² - (1/3)x + 1, and the quotient so far is (1/3)x. Now, the remainder's degree (2) is still equal to the denominator's degree, so we can divide again. Divide x² by 3x², which gives 1/3. Multiply the denominator by 1/3: (1/3)(3x² - 3x +4) = x² - x + 4/3. Subtract this from the current remainder:

(x² - (1/3)x + 1) - (x² - x + 4/3) = [0x²] + (2/3)x - (1/3).

So now the new remainder is (2/3)x - 1/3, and the quotient is (1/3)x + 1/3. Therefore, the original integrand can be written as:

(1/3)x + 1/3 + [(2/3)x - 1/3]/(3x² - 3x +4).

So the integral becomes the integral of (1/3)x + 1/3 plus the integral of [(2/3)x - 1/3]/(3x² -3x +4) dx. Let's split this into two parts: the polynomial part and the remaining fraction.

First, integrate (1/3)x + 1/3 from 0 to 1. That's straightforward. The integral of (1/3)x is (1/6)x², and the integral of 1/3 is (1/3)x. Evaluated from 0 to 1, that would be (1/6)(1)^2 + (1/3)(1) - [0 + 0] = 1/6 + 1/3 = 1/6 + 2/6 = 3/6 = 1/2. So the first part is 1/2.

Now, the second integral: ∫[(2/3)x - 1/3]/(3x² -3x +4) dx from 0 to1. Let's simplify this. Let me factor out 1/3 from the numerator: (1/3)∫[2x -1]/[3x² -3x +4] dx. So the integral becomes (1/3) times the integral of (2x -1)/(3x² -3x +4) dx.

Hmm, the denominator's derivative is 6x -3. Let me check: d/dx (3x² -3x +4) = 6x -3. The numerator here is 2x -1. Let's see if we can express 2x -1 as a multiple of the derivative. Let's see: 6x -3 is 3*(2x -1). So 2x -1 is (1/3)(6x -3). Therefore, the integral becomes (1/3) * ∫ [ (1/3)(6x -3) ] / (3x² -3x +4) dx. That simplifies to (1/9) ∫ (6x -3)/(3x² -3x +4) dx.

This is helpful because the numerator is the derivative of the denominator. Let me set u = 3x² -3x +4, then du/dx = 6x -3, so du = (6x -3) dx. Therefore, the integral becomes (1/9) ∫ du/u. Which is (1/9) ln|u| + C. So substituting back, we get (1/9) ln|3x² -3x +4|. Evaluated from 0 to1.

So the second part of the integral is (1/9)[ln(3(1)^2 -3(1) +4) - ln(3(0)^2 -3(0) +4)] = (1/9)[ln(3 -3 +4) - ln(4)] = (1/9)[ln(4) - ln(4)]? Wait, that can't be right. Wait, 3(1)^2 -3(1) +4 is 3 -3 +4 =4, and 3(0)^2 -3(0 +4 is 4. So ln(4) - ln(4) is zero? That would make the second integral zero? But that can't be. Wait, but wait, let me check the steps again.

Wait, the integral of (2x -1)/(3x² -3x +4) dx was transformed by expressing 2x -1 as (1/3)(6x -3), which is correct. Then the integral becomes (1/9) ∫ du/u, which is (1/9) ln|u|. So when evaluated from 0 to1, it's (1/9)(ln(4) - ln(4)) = 0. So the second integral is zero? That seems odd. But according to the calculation, yes. Wait, but that would mean the entire integral is just 1/2 + 0 = 1/2. But that seems too simple. Let me check again.

Wait, perhaps I made a mistake in the polynomial division. Let me verify that. Original integrand: (x³ +x +1)/(3x² -3x +4). Let's perform the division again. Divide x³ by 3x², which gives (1/3)x. Multiply denominator by (1/3)x: (1/3)x*(3x² -3x +4) = x³ -x² + (4/3)x. Subtract this from the numerator: (x³ +x +1) - (x³ -x² +4/3x) = 0 +x² - (1/3)x +1. So the remainder is x² - (1/3)x +1. Then, divide this by the denominator 3x² -3x +4. The leading term is x² divided by 3x², which is 1/3. Multiply denominator by 1/3: 1/3*(3x² -3x +4) = x² -x +4/3. Subtract this from the remainder: (x² -1/3x +1) - (x² -x +4/3) = (0x²) + (2/3x) -1/3. So the remainder is (2/3)x -1/3. Therefore, the division is correct. So the integrand is (1/3)x +1/3 + (2/3x -1/3)/(3x² -3x +4). Then, when integrating, the second part is (1/3)x +1/3, which integrates to 1/6x² +1/3x. Evaluated from 0 to1 gives 1/6 +1/3 =1/2. Then the remaining integral is (1/3)∫(2x -1)/(3x² -3x +4) dx. Then, as before, we note that the derivative of the denominator is 6x -3, which is 3*(2x -1). Therefore, (2x -1) is (1/3)(6x -3). So the integral becomes (1/3)*(1/3)∫(6x -3)/(3x² -3x +4) dx = (1/9) ln|3x² -3x +4| from 0 to1. But at x=1, denominator is 4, at x=0, denominator is 4. So ln(4) - ln(4) =0. Therefore, the entire integral is 1/2 +0 =1/2. But wait, that seems too straightforward. Let me check with a different approach.

Alternatively, maybe there's another term in the integral. Wait, perhaps after the polynomial division, the remainder is (2/3 -1/3) but maybe I missed a term. Wait, the remainder after division is (2/3)x -1/3. So the integrand is (1/3)x +1/3 + (2/3 -1/3)/(3x² -3x +4). Wait, but (2/3)x -1/3 over denominator. So when I split the integral into two parts: the first part is (1/3)x +1/3, which integrates to 1/2. The second part is ∫(2x -1)/(3x² -3x +4) dx multiplied by 1/3. Then, as before, that integral is (1/9)(ln(4) - ln(4)) =0. So the total integral is 1/2. But let's check with a different method. Let's compute the integral numerically to see if it's approximately 0.5. Let me do a quick approximation. Let's take x=0: the integrand is (0 +0 +1)/(0 -0 +4)=1/4=0.25. At x=1: (1 +1 +1)/(3 -3 +4)=3/4=0.75. The function is between 0.25 and 0.75, and the average around 0.5. So integrating from 0 to1, maybe the area is around 0.5. So 1/2 seems plausible. But let me check with another approach. Alternatively, maybe there's a mistake in assuming that the entire integral of the second part is zero. Let me compute the integral of (2x -1)/(3x² -3x +4) dx. Let me compute the antiderivative. Let me set u =3x² -3x +4. Then du/dx=6x -3. So (2x -1) dx is (1/3) du. Therefore, ∫(2x -1)/u dx = (1/3)∫du/u = (1/3) ln|u| +C. Therefore, the integral from 0 to1 is (1/3)(ln(4) - ln(4))=0. So yes, that part is zero. Therefore, the total integral is indeed 1/2. So the exact answer is 1/2, and the numerical approximation is 0.5. But wait, let me check with another method. Let me compute the integral numerically. Let's approximate the integral using the trapezoidal rule with a few intervals. Let's take x=0: 0.25, x=0.5: (0.125 +0.5 +1)/(3*(0.25) -1.5 +4)= (1.625)/(3*0.25=0.75; 0.75 -1.5= -0.75 +4=3.25. So 1.625/3.25=0.5. At x=0.5, the value is 0.5. At x=1, 0.75. So trapezoidal estimate with three points: (0.25 + 2*0.5 +0.75)/4 *1 = (0.25 +1 +0.75)/4=2/4=0.5. So the trapezoidal rule with two intervals gives 0.5. So that supports the analytical result. Therefore, the integral is indeed 1/2. So the exact answer is 1/2, and the numerical approximation is 0.5. Therefore, the final answer should be {"answer": "\\frac{1}{2}", "numerical_answer": "0.5000000000"}.
</think>

{"answer": "\\frac{1}{2}", "numerical_answer": "0.5000000000"}