
To solve the definite integral \(\int\limits_0^1 x^{-1} \ln x \ln \frac{2+x}{2-x} \, dx\), we proceed as follows:

### Step 1: Simplify the Integrand
First, expand the logarithm of the quotient:
\[
\ln \frac{2+x}{2-x} = \ln(2+x) - \ln(2-x)
\]
Thus, the integral becomes:
\[
\int_0^1 \frac{\ln x}{x} \left[ \ln(2+x) - \ln(2-x) \right] dx
\]

### Step 2: Split the Integral
Split the integral into two parts:
\[
I = \int_0^1 \frac{\ln x}{x} \ln(2+x) \, dx - \int_0^1 \frac{\ln x}{x} \ln(2-x) \, dx
\]

### Step 3: Expand Logarithms as Power Series
Express \(\ln(2+x)\) and \(\ln(2-x)\) using power series. For \(|x/2| < 1\) (which holds for \(x \in [0,1]\)):
\[
\ln(2+x) = \ln 2 + \ln\left(1 + \frac{x}{2}\right) = \ln 2 + \sum_{n=1}^\infty \frac{(-1)^{n+1}}{n} \left( \frac{x}{2} \right)^n
\]
\[
\ln(2-x) = \ln 2 + \ln\left(1 - \frac{x}{2}\right) = \ln 2 + \sum_{n=1}^\infty \frac{-1}{n} \left( \frac{x}{2} \right)^n
\]

### Step 4: Substitute and Simplify
Substituting these into the integral, the \(\ln 2\) terms cancel, leaving:
\[
I = \int_0^1 \frac{\ln x}{x} \left[ \sum_{n=1}^\infty \frac{(-1)^{n+1}}{n} \left( \frac{x}{2} \right)^n - \sum_{n=1}^\infty \frac{-1}{n} \left( \frac{x}{2} \right)^n \right] dx
\]
Simplifying the series:
\[
I = \sum_{n=1}^\infty \frac{1}{n \cdot 2^n} \left[ (-1)^{n+1} + 1 \right] \int_0^1 x^{n-1} \ln x \, dx
\]

### Step 5: Evaluate the Integral of \(x^{n-1} \ln x\)
The integral \(\int_0^1 x^{n-1} \ln x \, dx = -\frac{1}{n^2}\) (verified via integration by parts).

### Step 6: Simplify the Series
For even \(n\), \((-1)^{n+1} + 1 = 0\). For odd \(n = 2k+1\), \((-1)^{n+1} + 1 = 2\). Thus:
\[
I = -\sum_{k=0}^\infty \frac{1}{(2k+1)^3 4^k}
\]

### Step 7: Relate to Polylogarithms
This series is equivalent to \(I = \text{Li}_3\left(-\frac{1}{2}\right) - \text{Li}_3\left(\frac{1}{2}\right)\), where \(\text{Li}_3(z)\) is the trilogarithm function.

### Numerical Approximation
Using known values of the trilogarithm:
\[
\text{Li}_3\left(\frac{1}{2}\right) \approx 0.83564884805, \quad \text{Li}_3\left(-\frac{1}{2}\right) \approx -0.17416300005
\]
Thus:
\[
I \approx -0.17416300005 - 0.83564884805 = -1.0098118481
\]

### Final Answer
The exact answer is \(\text{Li}_3\left(-\frac{1}{2}\right) - \text{Li}_3\left(\frac{1}{2}\right)\), and the numerical approximation is \(-1.0098118481\).

{"answer": "\(\text{Li}_3\left(-\frac{1}{2}\right) - \text{Li}_3\left(\frac{1}{2}\right)\)", "numerical_answer": "-1.0098118481"}