Let's evaluate the definite integral:
\[
I = \int_0^1 \left( \frac{x^2}{2-x^2} + \sqrt{\frac{2x}{x+1}} \right)\,dx
\]
We'll split this into two parts:
\[
I = I_1 + I_2
\]
where
\[
I_1 = \int_0^1 \frac{x^2}{2-x^2}\,dx, \qquad I_2 = \int_0^1 \sqrt{\frac{2x}{x+1}}\, dx
\]

---

### Step 1: Compute \( I_1 = \int_0^1 \frac{x^2}{2-x^2}\,dx \)

First, rewrite the integrand as:
\[
\frac{x^2}{2-x^2} = \frac{2 - (2 - x^2)}{2-x^2} = 1 - \frac{2}{2-x^2}
\]
So,
\[
I_1 = \int_0^1 1\,dx - 2\int_0^1 \frac{1}{2-x^2}\, dx
\]

Calculate each term:

- The first term: \( \int_0^1 1\,dx = 1 \).

- The second term:

Letâ€™s compute \( J = \int_0^1 \frac{1}{2-x^2}\,dx \):

We can write:
\[
\frac{1}{2-x^2} = \frac{1}{(\sqrt{2}-x)(\sqrt{2}+x)}
\]
But it is easier to factor as:
\[
2 - x^2 = (\sqrt{2} - x)(\sqrt{2} + x)
\]

We can use the standard integral:

\[
\int \frac{1}{a^2 - x^2}\,dx = \frac{1}{2a} \ln\left|\frac{a+x}{a-x}\right| + C, \quad a > 0
\]

So for \( a = \sqrt{2} \):

\[
J = \int_0^1 \frac{1}{2-x^2}\,dx 
= \frac{1}{2\sqrt{2}} \left[ \ln \left| \frac{\sqrt{2}+x}{\sqrt{2}-x} \right| \right]_0^1
\]
\[
= \frac{1}{2\sqrt{2}} \left( \ln \left( \frac{\sqrt{2}+1}{\sqrt{2}-1} \right) - \ln \left( \frac{\sqrt{2}+0}{\sqrt{2}-0} \right) \right)
\]
\[
= \frac{1}{2\sqrt{2}} \ln \left( \frac{\sqrt{2}+1}{\sqrt{2}-1} \cdot \frac{\sqrt{2}}{\sqrt{2}+0} \right)
\]

But actually,
\[
\ln \left( \frac{\sqrt{2}+1}{\sqrt{2}-1} \right) - \ln \left( \frac{\sqrt{2}+0}{\sqrt{2}-0} \right) = \ln \left( \frac{\sqrt{2}+1}{\sqrt{2}-1} \cdot \frac{\sqrt{2}-0}{\sqrt{2}+0} \right)
\]
But \( \frac{\sqrt{2}}{\sqrt{2}}=1 \), so that drops out.

So the antiderivative is:
\[
J = \frac{1}{2\sqrt{2}} \left[ \ln \left( \frac{\sqrt{2}+x}{\sqrt{2}-x} \right) \right]_{x=0}^{x=1}
\]
So
\[
J = \frac{1}{2\sqrt{2}}\left( \ln \left( \frac{\sqrt{2}+1}{\sqrt{2}-1} \right) - \ln \left( \frac{\sqrt{2}}{\sqrt{2}} \right) \right)
\]
\[
= \frac{1}{2\sqrt{2}}\ln \left( \frac{\sqrt{2}+1}{\sqrt{2}-1} \right)
\]

So,
\[
I_1 = 1 - 2J = 1 - \frac{1}{\sqrt{2}} \ln\left( \frac{\sqrt{2}+1}{\sqrt{2}-1} \right)
\]

---

### Step 2: Compute \( I_2 = \int_0^1 \sqrt{\frac{2x}{x+1}}\, dx \)

Set \( x = t^2 \), so that when \( x = 0 \), \( t = 0 \), and when \( x = 1 \), \( t = 1 \).
Then,
\[
dx = 2t\,dt
\]
and
\[
\sqrt{\frac{2x}{x+1}} = \sqrt{ \frac{2t^2}{t^2 + 1} } = t \sqrt{ \frac{2}{t^2 + 1} }
\]

Therefore,
\[
I_2 = \int_{x=0}^{x=1} \sqrt{ \frac{2x}{x+1}} dx = \int_{t=0}^{t=1} t \sqrt{ \frac{2}{t^2 + 1} } \cdot 2t\,dt = 2 \int_0^1 t^2 \left( \frac{2}{t^2+1} \right)^{1/2} dt
\]
\[
= 2\sqrt{2} \int_0^1 \frac{t^2}{(t^2+1)^{1/2}} dt
\]

Let's compute \( K = \int_0^1 \frac{t^2}{(t^2+1)^{1/2}} dt \).

We can write \( t^2 = (t^2+1) - 1 \), so:
\[
\frac{t^2}{\sqrt{t^2+1}} = \frac{t^2+1}{\sqrt{t^2+1}} - \frac{1}{\sqrt{t^2+1}} = \sqrt{t^2+1} - \frac{1}{\sqrt{t^2+1}}
\]

So
\[
K = \int_0^1 \sqrt{t^2+1}\,dt - \int_0^1 \frac{dt}{\sqrt{t^2+1}}
\]

Both integrals are standard:

- \( \int \sqrt{t^2+1}\,dt = \frac{1}{2} (t\sqrt{t^2+1} + \ln(t+\sqrt{t^2+1})) + C \)

- \( \int \frac{dt}{\sqrt{t^2+1}} = \operatorname{arcsinh}(t) + C = \ln(t+\sqrt{t^2+1}) + C \)

Therefore,

\[
K = \left[ \frac{1}{2} ( t\sqrt{t^2+1} + \ln(t+\sqrt{t^2+1}) ) - \ln(t+\sqrt{t^2+1}) \right]_0^1
\]
\[
= \left[ \frac{1}{2} t\sqrt{t^2+1} - \frac{1}{2} \ln(t+\sqrt{t^2+1}) \right]_0^1
\]

Let's evaluate at \( t=1 \):
- \( t\sqrt{t^2+1} = 1 \cdot \sqrt{2} = \sqrt{2} \)
- \( t+\sqrt{t^2+1} = 1 + \sqrt{2} \)

At \( t=0 \):
- \( t\sqrt{t^2+1} = 0 \)
- \( t+\sqrt{t^2+1} = 0 + 1 = 1 \)

So:

\[
K = \frac{1}{2} \left( \sqrt{2} - 0 \right) - \frac{1}{2} \left( \ln(1+\sqrt{2}) - \ln(1) \right )
= \frac{\sqrt{2}}{2} - \frac{1}{2}\ln(1+\sqrt{2})
\]

Recall,
\[
I_2 = 2\sqrt{2} K = 2\sqrt{2}\left( \frac{\sqrt{2}}{2} - \frac{1}{2}\ln(1+\sqrt{2}) \right ) = 2\sqrt{2} \cdot \frac{\sqrt{2}}{2} - 2\sqrt{2} \cdot \frac{1}{2}\ln(1+\sqrt{2})
= 2 - \sqrt{2}\ln(1+\sqrt{2})
\]

---

### Step 3: Put it Together

The total integral is:
\[
I = I_1 + I_2 =
\left[ 1 - \frac{1}{\sqrt{2}}\ln \left( \frac{\sqrt{2}+1}{\sqrt{2}-1}\right) \right ] + \left[ 2 - \sqrt{2}\ln(1+\sqrt{2}) \right ]
\]
\[
= 3 - \frac{1}{\sqrt{2}}\ln \left( \frac{\sqrt{2}+1}{\sqrt{2}-1} \right ) - \sqrt{2}\ln(1+\sqrt{2})
\]

---

### Step 4: Compute Numerical Answer

Let's compute each term numerically:

1. \(\sqrt{2} = 1.4142135624\)
2. \(1+\sqrt{2} = 2.4142135624\)
3. \(1-\sqrt{2} = -0.4142135624\)
4. \(\sqrt{2}+1 = 2.4142135624\)
5. \(\sqrt{2}-1 = 0.4142135624\)

So,
\[
\frac{\sqrt{2}+1}{\sqrt{2}-1} = \frac{2.4142135624}{0.4142135624} \approx 5.8284271248
\]
- \(\ln(5.8284271248) \approx 1.7627471740\)

- \(\ln(2.4142135624) \approx 0.8813735870\)

Now,
- \(1/\sqrt{2} = 0.7071067812\)
- \(\sqrt{2} = 1.4142135624\)

So:

- \( 0.7071067812 \times 1.7627471740 \approx 1.2464393532 \)
- \(1.4142135624 \times 0.8813735870 \approx 1.2464393532\) (interesting: they agree very closely!)

So,
- \(I = 3 - 1.2464393532 - 1.2464393532\)
- \(I = 3 - 2.4928787064\)
- \(I = 0.5071212936\)

Rounded to 10 decimal places: **0.5071212936**

---

### Final JSON Output

```json
{"answer": "3 - \\frac{1}{\\sqrt{2}}\\ln\\left(\\frac{\\sqrt{2}+1}{\\sqrt{2}-1}\\right) - \\sqrt{2}\\ln(1+\\sqrt{2})", "numerical_answer": "0.5071212936"}
```