# Evaluating $\int\limits_{0}^{2}x^{1/4}(2-x)^{-1/4}\cosh\left(1\sqrt[4]{x(2-x)}\right)dx$

## Step 1: Substitution

Let's use the substitution $u = \sqrt[4]{x(2-x)}$. First, we need to find how $x$ relates to $u$.

We have $u^4 = x(2-x) = 2x - x^2$

This gives us $x^2 - 2x + u^4 = 0$

Using the quadratic formula:
$x = \frac{2 \pm \sqrt{4-4u^4}}{2} = 1 \pm \sqrt{1-u^4}$

When $x = 0$, we have $u = 0$
When $x = 2$, we have $u = 0$

As $x$ increases from $0$ to $1$, $u$ increases from $0$ to $1$
As $x$ increases from $1$ to $2$, $u$ decreases from $1$ to $0$

We need to find $dx$ in terms of $u$:
$\frac{dx}{du} = \frac{d}{du}(1 \pm \sqrt{1-u^4})$

For $0 \leq x \leq 1$, we use $x = 1 - \sqrt{1-u^4}$, so:
$\frac{dx}{du} = \frac{4u^3}{2\sqrt{1-u^4}}$

For $1 \leq x \leq 2$, we use $x = 1 + \sqrt{1-u^4}$, so:
$\frac{dx}{du} = -\frac{4u^3}{2\sqrt{1-u^4}} = -\frac{2u^3}{\sqrt{1-u^4}}$

## Step 2: Express the integrand in terms of $u$

We need to express $x^{1/4}(2-x)^{-1/4}$ in terms of $u$.

$x(2-x) = u^4$ implies $x^{1/4}(2-x)^{1/4} = u$

Therefore, $x^{1/4}(2-x)^{-1/4} = \frac{x^{1/4}}{(2-x)^{1/4}} = \frac{u}{(2-x)^{1/2}}$

We know that $2-x = 1 + \sqrt{1-u^4}$ for $0 \leq x \leq 1$
And $2-x = 1 - \sqrt{1-u^4}$ for $1 \leq x \leq 2$

## Step 3: Compute the integral

Analyzing this integral further, I notice we can use symmetry. The integral from $0$ to $2$ can be split into two parts:
$\int_{0}^{1} + \int_{1}^{2}$

Due to the symmetry around $x = 1$, these two integrals are equal. So:
$\int_{0}^{2} = 2\int_{0}^{1}$

For the $u$-substitution, as $x$ goes from $0$ to $1$, $u$ goes from $0$ to $1$.

When we substitute, we get:
$\int_{0}^{1} x^{1/4}(2-x)^{-1/4}\cosh(u)dx$

Now, with the substitution, we get:
$\int_{0}^{1} \cosh(u) \cdot 2u \cdot du = 2\int_{0}^{1} u\cosh(u)du$

## Step 4: Evaluate the resulting integral

$2\int_{0}^{1} u\cosh(u)du$

We can use integration by parts with $dv = \cosh(u)du$ and $v = \sinh(u)$:
$2\int_{0}^{1} u\cosh(u)du = 2[u\sinh(u)]_{0}^{1} - 2\int_{0}^{1} \sinh(u)du$
$= 2 \cdot 1 \cdot \sinh(1) - 2 \cdot 0 \cdot \sinh(0) - 2[\cosh(u)]_{0}^{1}$
$= 2\sinh(1) - 2[\cosh(1) - \cosh(0)]$
$= 2\sinh(1) - 2\cosh(1) + 2$
$= 2(1 + \sinh(1) - \cosh(1))$

## Step 5: Numerical approximation

$\sinh(1) \approx 1.1752011936438014$
$\cosh(1) \approx 1.5430806348152437$

Therefore:
$2(1 + \sinh(1) - \cosh(1)) = 2(1 + 1.1752011936438014 - 1.5430806348152437)$
$= 2(0.6321205588285577) = 1.2642411176571154$

Rounded to 10 decimal places: $1.2642411177$

## Final Answer

The exact value of the integral is $2(1 + \sinh(1) - \cosh(1))$

{"answer": "2(1 + \\sinh(1) - \\cosh(1))", "numerical_answer": "1.2642411177"}