# Calculating $\int_1^\infty\frac{\log x}{x^2}dx$

## Step 1: Set up the integral
I'll compute $\int_1^\infty\frac{\log x}{x^2}dx$

## Step 2: Use substitution
Let $u = \log x$, which means $x = e^u$ and $dx = e^u du$

When $x = 1$, $u = \log(1) = 0$
When $x \to \infty$, $u \to \infty$

Rewriting the integral:
$\int_1^\infty\frac{\log x}{x^2}dx = \int_0^\infty\frac{u}{(e^u)^2}e^u du = \int_0^\infty u e^{-u} du$

## Step 3: Integration by parts
I'll use integration by parts with:
- $f(u) = u$, so $f'(u) = 1$
- $g'(u) = e^{-u}$, so $g(u) = -e^{-u}$

The formula is: $\int f(u)g'(u)du = f(u)g(u) - \int f'(u)g(u)du$

Thus:
$\int_0^\infty u e^{-u} du = \left[ -u e^{-u} \right]_0^\infty - \int_0^\infty (-e^{-u}) \cdot 1 du$

$= \left[ -u e^{-u} \right]_0^\infty + \int_0^\infty e^{-u} du$

## Step 4: Evaluate the terms
For the first term:
- As $u \to \infty$, $-u e^{-u} \to 0$ (by L'HÃ´pital's rule)
- At $u = 0$, $-u e^{-u} = 0$

So $\left[ -u e^{-u} \right]_0^\infty = 0 - 0 = 0$

For the second term:
$\int_0^\infty e^{-u} du = \left[ -e^{-u} \right]_0^\infty = 0 - (-1) = 1$

## Step 5: Combine results
$\int_1^\infty\frac{\log x}{x^2}dx = 0 + 1 = 1$

## Step 6: Numerical approximation
The exact answer is 1, so the numerical approximation is 1.0000000000

{"answer": "1", "numerical_answer": "1.0000000000"}