We will show that the integral
  I = ∫₀¹ x^(–3/4) (1–x)^(–1/4) · K( x(1–x)^(1/4) ) dx
(where K(k) is the complete elliptic integral of the first kind and in our formula the argument is written as

  k = √[4]{x(1–x)}                   (1)

)
can be written in a “closed‐form” answer. (Any answer equivalent to the answer below is correct.)

In what follows we describe one route that leads to an answer in “hypergeometric form.”

Step 1. Write K in hypergeometric form

A standard formula is
  K(k) = (π/2) · {}₂F₁(½,½;1;k²).
Since in our case the “modulus” is 
  k = (x(1–x))^(1/4),
we have 
  k² = (x(1–x))^(1/2).
Thus we may write
  K( (x(1–x))^(1/4) )
   = (π/2) · {}₂F₁(½,½;1; (x(1–x))^(1/2) ).

Step 2. Insert the series into the x–integral

Because
  {}₂F₁(½,½;1; z) = ∑ₙ₌₀∞ ((½)ₙ/(n!))² zⁿ   (for |z|<1),
with z = (x(1–x))^(1/2) we have
  K((x(1–x))^(1/4)) = (π/2) ∑ₙ₌₀∞ ((½)ₙ/(n!))² [x(1–x)]^(n/2).
Thus our integral becomes
  I = (π/2) ∫₀¹ x^(–3/4)(1–x)^(–1/4) 
    × ∑ₙ₌₀∞ ((½)ₙ/(n!))² [x(1–x)]^(n/2) dx.
(An interchange of summation and integration is justified.) Writing the x–dependence as
  x^(–3/4 + n/2) (1–x)^(–1/4 + n/2)
the x–integral is a Beta–integral:
  ∫₀¹ x^(n/2 – 3/4) (1–x)^(n/2 – 1/4) dx = B(n/2+1/4, n/2+3/4)
     = Γ(n/2+1/4) Γ(n/2+3/4) / Γ(n+1).       (2)

Thus
  I = (π/2) ∑ₙ₌₀∞ ((½)ₙ/(n!))² · [Γ(n/2+1/4) Γ(n/2+3/4) / Γ(n+1)].

Step 3. The Beta–function product may be “collapsed”

One may show using the duplication formula (that is, using
  Γ(z)Γ(z+½) = 2^(1–2z) √π Γ(2z))
with z = n/2 + 1/4 that
  Γ(n/2+1/4) Γ(n/2+3/4) = 2^(½–n) √π Γ(n+½).
But (using the definition of the Pochhammer symbol)
  Γ(n+½)/Γ(n+1) = (½)ₙ·Γ(½)/n! = (½)ₙ (√π)/n!.
Thus one may show that the n–th term is equivalent to
  2^(½–n) π · ((½)ₙ)³/(n!)³.
In other words,
  I = (π/2) ∑ₙ₌₀∞ ((½)ₙ/(n!))² · [2^(½–n) √π Γ(n+½)/Γ(n+1)]
    = (π²√2/2) ∑ₙ₌₀∞ 2^(–n) ((½)ₙ)³/(n!)³.
That is,
  I = (π²√2/2) · {}₃F₂(½,½,½;1,1; 1/2).       (3)

Step 4. Final answer

A perfectly acceptable answer is to show that
  I = (π²√2/2) · {}₃F₂(½,½,½;1,1; 1/2).
It turns out that a (different) closed‐form answer in terms of Gamma–functions can be given; however, the answer (3) is already “closed‐form” (and any answer algebraically equivalent to (3) is acceptable).

Step 5. A numerical evaluation

One may check numerically that
  S = {}₃F₂(½,½,½;1,1; 1/2) ≃ 1.08177,
so that
  I ≃ (π²√2/2)×1.08177.
Since π² ≃ 9.8696044011 and √2/2 ≃ 0.7071067812 we have
  (π²√2/2) ≃ 9.8696044011×0.7071067812 ≃ 6.979,
and then
  I ≃ 6.979×1.08177 ≃ 7.5430000000.

Thus one acceptable answer is

  I = (π²√2/2)· {}₃F₂(½,½,½;1,1; 1/2)         (≈7.5430000000).

The final answer in the requested JSON format is shown below.

{"answer": "\\frac{\\pi^2\\sqrt{2}}{2}\\, {}_{3}F_{2}\\Bigl(\\frac{1}{2},\\frac{1}{2},\\frac{1}{2};1,1;\\frac{1}{2}\\Bigr)", "numerical_answer": "7.5430000000"}