To solve the definite integral \(\int_{0}^{1} \frac{x^{3} + x + 1}{3x^{2} - 3x + 4} \, dx\), we follow these steps:

### Step 1: Polynomial Long Division
First, observe that the degree of the numerator (3) is higher than the degree of the denominator (2). We perform polynomial long division to simplify the integrand:

\[
\frac{x^{3} + x + 1}{3x^{2} - 3x + 4}
\]

Divide \(x^3\) by \(3x^2\) to get \(\frac{x}{3}\). Multiply the denominator by \(\frac{x}{3}\) and subtract from the numerator:

\[
x^3 + x + 1 - \left(\frac{x}{3} \cdot (3x^2 - 3x + 4)\right) = x^3 + x + 1 - (x^3 - x^2 + \frac{4x}{3}) = x^2 - \frac{x}{3} + 1
\]

Now, divide \(x^2\) by \(3x^2\) to get \(\frac{1}{3}\). Multiply the denominator by \(\frac{1}{3}\) and subtract:

\[
x^2 - \frac{x}{3} + 1 - \left(\frac{1}{3} \cdot (3x^2 - 3x + 4)\right) = x^2 - \frac{x}{3} + 1 - (x^2 - x + \frac{4}{3}) = \frac{2x}{3} - \frac{1}{3}
\]

Thus, the integrand can be rewritten as:

\[
\frac{x^{3} + x + 1}{3x^{2} - 3x + 4} = \frac{x}{3} + \frac{1}{3} + \frac{\frac{2x}{3} - \frac{1}{3}}{3x^{2} - 3x + 4}
\]

Simplify the remainder term:

\[
\frac{\frac{2x}{3} - \frac{1}{3}}{3x^{2} - 3x + 4} = \frac{2x - 1}{9x^{2} - 9x + 12}
\]

### Step 2: Integrate Term by Term
Now, the integral becomes:

\[
\int_{0}^{1} \left(\frac{x}{3} + \frac{1}{3} + \frac{2x - 1}{9x^{2} - 9x + 12}\right) dx
\]

Integrate each term separately:

1. \(\int \frac{x}{3} \, dx = \frac{x^2}{6}\)
2. \(\int \frac{1}{3} \, dx = \frac{x}{3}\)
3. For the remaining term, let \(u = 9x^2 - 9x + 12\), then \(du = (18x - 9) dx = 9(2x - 1) dx\). Notice that the numerator is \(2x - 1\), so:

\[
\int \frac{2x - 1}{9x^{2} - 9x + 12} dx = \frac{1}{9} \int \frac{du}{u} = \frac{1}{9} \ln|u| + C = \frac{1}{9} \ln(9x^2 - 9x + 12) + C
\]

Combine all the terms:

\[
\int \frac{x^{3} + x + 1}{3x^{2} - 3x + 4} dx = \frac{x^2}{6} + \frac{x}{3} + \frac{1}{9} \ln(9x^2 - 9x + 12) + C
\]

### Step 3: Evaluate the Definite Integral
Evaluate from 0 to 1:

At \(x = 1\):

\[
\frac{1^2}{6} + \frac{1}{3} + \frac{1}{9} \ln(9(1)^2 - 9(1) + 12) = \frac{1}{6} + \frac{1}{3} + \frac{1}{9} \ln(12) = \frac{1}{2} + \frac{1}{9} \ln(12)
\]

At \(x = 0\):

\[
\frac{0^2}{6} + \frac{0}{3} + \frac{1}{9} \ln(9(0)^2 - 9(0) + 12) = \frac{1}{9} \ln(12)
\]

Subtract the lower limit from the upper limit:

\[
\left(\frac{1}{2} + \frac{1}{9} \ln(12)\right) - \left(\frac{1}{9} \ln(12)\right) = \frac{1}{2}
\]

### Step 4: Numerical Approximation
The exact answer is \(\frac{1}{2}\), which numerically is \(0.5000000000\).

### Final Answer
```json
{"answer": "\\frac{1}{2}", "numerical_answer": "0.5000000000"}
```