# Evaluating the Definite Integral $\int_0^{\frac{1}{2}}\left\lfloor\frac{1}{x}\right\rfloor\left\lceil\frac{1}{x}\right\rceil\ln\left(1-\frac{1}{\left\lfloor\frac{1}{x}\right\rfloor^2}\right)\mathrm{d}x$

## Step 1: Identify the behavior of the floor and ceiling functions

First, I'll identify the intervals where $\left\lfloor\frac{1}{x}\right\rfloor$ and $\left\lceil\frac{1}{x}\right\rceil$ are constant.

For $x \in (0,\frac{1}{2}]$:
- When $x \in (\frac{1}{n+1}, \frac{1}{n}]$, we have $\left\lfloor\frac{1}{x}\right\rfloor = n$ and $\left\lceil\frac{1}{x}\right\rceil = n+1$ for $n = 2, 3, 4, ...$
- At the boundary points $x = \frac{1}{n}$, we have $\left\lfloor\frac{1}{x}\right\rfloor = \left\lceil\frac{1}{x}\right\rceil = n$, but these points have measure zero.

## Step 2: Rewrite the integral as a sum

The integral can be rewritten as:
$$\int_0^{\frac{1}{2}}\left\lfloor\frac{1}{x}\right\rfloor\left\lceil\frac{1}{x}\right\rceil\ln\left(1-\frac{1}{\left\lfloor\frac{1}{x}\right\rfloor^2}\right)\mathrm{d}x = \sum_{n=2}^{\infty}\int_{\frac{1}{n+1}}^{\frac{1}{n}}n(n+1)\ln\left(1-\frac{1}{n^2}\right)\mathrm{d}x$$

## Step 3: Evaluate the integrals in the sum

For each term in the sum:
$$\int_{\frac{1}{n+1}}^{\frac{1}{n}}n(n+1)\ln\left(1-\frac{1}{n^2}\right)\mathrm{d}x = n(n+1)\ln\left(1-\frac{1}{n^2}\right)\left[\frac{1}{n} - \frac{1}{n+1}\right]$$

$$= n(n+1)\ln\left(1-\frac{1}{n^2}\right)\left[\frac{1}{n(n+1)}\right]$$

$$= \ln\left(1-\frac{1}{n^2}\right)$$

$$= \ln\left(\frac{n^2-1}{n^2}\right)$$

$$= \ln\left(\frac{(n-1)(n+1)}{n^2}\right)$$

$$= \ln\left(\frac{n-1}{n}\cdot\frac{n+1}{n}\right)$$

$$= \ln\left(\frac{n-1}{n}\right) + \ln\left(\frac{n+1}{n}\right)$$

$$= \ln\left(1-\frac{1}{n}\right) + \ln\left(1+\frac{1}{n}\right)$$

## Step 4: Compute the sum

The integral becomes:
$$\sum_{n=2}^{\infty}\left[\ln\left(1-\frac{1}{n}\right) + \ln\left(1+\frac{1}{n}\right)\right]$$

Let's examine the partial sums:
$$S_N = \sum_{n=2}^{N}\left[\ln\left(1-\frac{1}{n}\right) + \ln\left(1+\frac{1}{n}\right)\right]$$

$$= \sum_{n=2}^{N}\ln\left(1-\frac{1}{n}\right) + \sum_{n=2}^{N}\ln\left(1+\frac{1}{n}\right)$$

For the first sum:
$$\sum_{n=2}^{N}\ln\left(1-\frac{1}{n}\right) = \sum_{n=2}^{N}\ln\left(\frac{n-1}{n}\right) = \sum_{n=2}^{N}\ln(n-1) - \sum_{n=2}^{N}\ln(n)$$

$$= \ln(1) + \ln(2) + ... + \ln(N-1) - \ln(2) - \ln(3) - ... - \ln(N)$$

$$= \ln(1) - \ln(N) = -\ln(N)$$

For the second sum:
$$\sum_{n=2}^{N}\ln\left(1+\frac{1}{n}\right) = \sum_{n=2}^{N}\ln\left(\frac{n+1}{n}\right) = \sum_{n=2}^{N}\ln(n+1) - \sum_{n=2}^{N}\ln(n)$$

$$= \ln(3) + \ln(4) + ... + \ln(N+1) - \ln(2) - \ln(3) - ... - \ln(N)$$

$$= \ln(N+1) - \ln(2) = \ln\left(\frac{N+1}{2}\right)$$

Combining the two sums:
$$S_N = -\ln(N) + \ln\left(\frac{N+1}{2}\right) = \ln\left(\frac{N+1}{2N}\right)$$

As $N \to \infty$, we have:
$$\lim_{N \to \infty}\ln\left(\frac{N+1}{2N}\right) = \ln\left(\frac{1}{2}\right) = -\ln(2)$$

## Step 5: Final result

The exact value of the definite integral is:
$$\int_0^{\frac{1}{2}}\left\lfloor\frac{1}{x}\right\rfloor\left\lceil\frac{1}{x}\right\rceil\ln\left(1-\frac{1}{\left\lfloor\frac{1}{x}\right\rfloor^2}\right)\mathrm{d}x = -\ln(2)$$

The numerical approximation of $-\ln(2)$ to 10 decimal places is:
$$-\ln(2) = -0.6931471806$$

{"answer": "-\\ln(2)", "numerical_answer": "-0.6931471806"}