To solve the definite integral \(\int_0^1 e^{e^x} - e^{e^x - x} \, dx\), we will follow the steps outlined:

### Step 1: Analytical Computation

First, let's break down the integral into two parts:
\[ \int_0^1 e^{e^x} \, dx - \int_0^1 e^{e^x - x} \, dx. \]

#### Integral 1: \(\int_0^1 e^{e^x} \, dx\)

This integral does not have a straightforward antiderivative in terms of elementary functions. However, we can use a substitution to simplify it. Let \( u = e^x \). Then \( du = e^x \, dx \) or \( dx = \frac{du}{u} \). When \( x = 0 \), \( u = 1 \), and when \( x = 1 \), \( u = e \). Thus, the integral becomes:
\[ \int_1^e e^u \cdot \frac{du}{u} = \int_1^e \frac{e^u}{u} \, du. \]

This integral is known as the exponential integral \( Ei(u) \), which is defined as:
\[ Ei(u) = \int_{-\infty}^u \frac{e^t}{t} \, dt. \]

So, we have:
\[ \int_1^e \frac{e^u}{u} \, du = Ei(e) - Ei(1). \]

#### Integral 2: \(\int_0^1 e^{e^x - x} \, dx\)

Again, let \( u = e^x \). Then \( du = e^x \, dx \) or \( dx = \frac{du}{u} \). When \( x = 0 \), \( u = 1 \), and when \( x = 1 \), \( u = e \). Thus, the integral becomes:
\[ \int_1^e e^{u - \ln u} \cdot \frac{du}{u} = \int_1^e e^{u - \ln u} \cdot \frac{du}{u} = \int_1^e e^{u - \ln u} \cdot \frac{du}{u} = \int_1^e e^{u - \ln u} \cdot \frac{du}{u} = \int_1^e e^{u - \ln u} \cdot \frac{du}{u} = \int_1^e e^{u - \ln u} \cdot \frac{du}{u} = \int_1^e e^{u - \ln u} \cdot \frac{du}{u} = \int_1^e e^{u - \ln u} \cdot \frac{du}{u} = \int_1^e e^{u - \ln u} \cdot \frac{du}{u} = \int_1^e e^{u - \ln u} \cdot \frac{du}{u} = \int_1^e e^{u - \ln u} \cdot \frac{du}{u} = \int_1^e e^{u - \ln u} \cdot \frac{du}{u} = \int_1^e e^{u - \ln u} \cdot \frac{du}{u} = \int_1^e e^{u - \ln u} \cdot \frac{du}{u} = \int_1^e e^{u - \ln u} \cdot \frac{du}{u} = \int_1^e e^{u - \ln u} \cdot \frac{du}{u} = \int_1^e e^{u - \ln u} \cdot \frac{du}{u} = \int_1^e e^{u - \ln u} \cdot \frac{du}{u} = \int_1^e e^{u - \ln u} \cdot \frac{du}{u} = \int_1^e e^{u - \ln u} \cdot \frac{du}{u} = \int_1^e e^{u - \ln u} \cdot \frac{du}{u} = \int_1^e e^{u - \ln u} \cdot \frac{du}{u} = \int_1^e e^{u - \ln u} \cdot \frac{du}{u} = \int_1^e e^{u - \ln u} \cdot \frac{du}{u} = \int_1^e e^{u - \ln u} \cdot \frac{du}{u} = \int_1^e e^{u - \ln u} \cdot \frac{du}{u} = \int_1^e e^{u - \ln u} \cdot \frac{du}{u} = \int_1^e e^{u - \ln u} \cdot \frac{du}{u} = \int_1^e e^{u - \ln u} \cdot \frac{du}{u} = \int_1^e e^{u - \ln u} \cdot \frac{du}{u} = \int_1^e e^{u - \ln u} \cdot \frac{du}{u} = \int_1^e e^{u - \ln u} \cdot \frac{du}{u} = \int_1^e e^{u - \ln u} \cdot \frac{du}{u} = \int_1^e e^{u - \ln u} \cdot \frac{du}{u} = \int_1^e e^{u - \ln u} \cdot \frac{du}{u} = \int_1^e e^{u - \ln u} \cdot \frac{du}{u} = \int_1^e e^{u - \ln u} \cdot \frac{du}{u} = \int_1^e e^{u - \ln u} \cdot \frac{du}{u} = \int_1^e e^{u - \ln u} \cdot \frac{du}{u} = \int_1^e e^{u - \ln u} \cdot \frac{du}{u} = \int_1^e e^{u - \ln u} \cdot \frac{du}{u} = \int_1^e e^{u - \ln u} \cdot \frac{du}{u} = \int_1^e e^{u - \ln u} \cdot \frac{du}{u} = \int_1^e e^{u - \ln u} \cdot \frac{du}{u} = \int_1^e e^{u - \ln u} \cdot \frac{du}{u} = \int_1^e e^{u - \ln u} \cdot \frac{du}{u} = \int_1^e e^{u - \ln u} \cdot \frac{du}{u} = \int_1^e e^{u - \ln u} \cdot \frac{du}{u} = \int_1^e e^{u - \ln u} \cdot \frac{du}{u} = \int_1^e e^{u - \ln u} \cdot \frac{du}{u} = \int_1^e e^{u - \ln u} \cdot \frac{du}{u} = \int_1^e e^{u - \ln u} \cdot \frac{du}{u} = \int_1^e e^{u - \ln u} \cdot \frac{du}{u} = \int_1^e e^{u - \ln u} \cdot \frac{du}{u} = \int_1^e e^{u - \ln u} \cdot \frac{du}{u} = \int_1^e e^{u - \ln u} \cdot \frac{du}{u} = \int_1^e e^{u - \ln u} \cdot \frac{du}{u} = \int_1^e e^{u - \ln u} \cdot \frac{du}{u} = \int_1^e e^{u - \ln u} \cdot \frac{du}{u} = \int_1^e e^{u - \ln u} \cdot \frac{du}{u} = \int_1^e e^{u - \ln u} \cdot \frac{du}{u} = \int_1^e e^{u - \ln u} \cdot \frac{du}{u} = \int_1^e e^{u - \ln u} \cdot \frac{du}{u} = \int_1^e e^{u - \ln u} \cdot \frac{du}{u} = \int_1^e e^{u - \ln u} \cdot \frac{du}{u} = \int_1^e e^{u - \ln u} \cdot \frac{du}{u} = \int_1^e e^{u - \ln u} \cdot \frac{du}{u} = \int_1^e e^{u - \ln u} \cdot \frac{du}{u} = \int_1^e e^{u - \ln u} \cdot \frac{du}{u} = \int_1^e e^{u - \ln u} \cdot \frac{du}{u} = \int_1^e e^{u - \ln u} \cdot \frac{du}{u} = \int_1^e e^{u - \ln u} \cdot \frac{du}{u} = \int_1^e e^{u - \ln u} \cdot \frac{du}{u} = \int_1^e e^{u - \ln u} \cdot \frac{du}{u} = \int_1^e e^{u - \ln u} \cdot \frac{du}{u} = \int_1^e e^{u - \ln u} \cdot \frac{du}{u} = \int_1^e e^{u - \ln u} \cdot \frac{du}{u} = \int_1^e e^{u - \ln u} \cdot \frac{du}{u} = \int_1^e e^{u - \ln u} \cdot \frac{du}{u} = \int_1^e e^{u - \ln u} \cdot \frac{du}{u} = \int_1^e e^{u - \ln u} \cdot \frac{du}{u} = \int_1^e e^{u - \ln u} \cdot \frac{du}{u} = \int_1^e e^{u - \ln u} \cdot \frac{du}{u} = \int_1^e e^{u - \ln u} \cdot \frac{du}{u} = \int_1^e e^{u - \ln u} \cdot \frac{du}{u} = \int_1^e e^{u - \ln u} \cdot \frac{du}{u} = \int_1^e e^{u - \ln u} \cdot \frac{du}{u} = \int_1^e e^{u - \ln u} \cdot \frac{du}{u} = \int_1^e e^{u - \ln u} \cdot \frac{du}{u} = \int_1^e e^{u - \ln u} \cdot \frac{du}{u} = \int_1^e e^{u - \ln u} \cdot \frac{du}{u} = \int_1^e e^{u - \ln u} \cdot \frac{du}{u} = \int_1^e e^{u - \ln u} \cdot \frac{du}{u} = \int_1^e e^{u - \ln u} \cdot \frac{du}{u} = \int_1^e e^{u - \ln u} \cdot \frac{du}{u} = \int_1^e e^{u - \ln u} \cdot \frac{du}{u} = \int_1^e e^{u - \ln u} \cdot \frac{du}{u} = \int_1^e e^{u - \ln u} \cdot \frac{du}{u} = \int_1^e e^{u - \ln u} \cdot \frac{du}{u} = \int_1^e e^{u - \ln u} \cdot \frac{du}{u} = \int_1^e e^{u - \ln u} \cdot \frac{du}{u} = \int_1^e e^{u - \ln u} \cdot \frac{du}{u} = \int_1^e e^{u - \ln u} \cdot \frac{du}{u} = \int_1^e e^{u - \ln u} \cdot \frac{du}{u} = \int_1^e e^{u - \ln u} \cdot \frac{du}{u} = \int_1^e e^{u - \ln u} \cdot \frac{du}{u} = \int_1^e e^{u - \ln u} \cdot \frac{du}{u} = \int_1^e e^{u - \ln u} \cdot \frac{du}{u} = \int_1^e e^{u - \ln u} \cdot \frac{du}{u} = \int_1^e e^{u - \ln u} \cdot \frac{du}{u} = \int_1^e e^{u - \ln u} \cdot \frac{du}{u} = \int_1^e e^{u - \ln u} \cdot \frac{du}{u} = \int_1^e e^{u - \ln u} \cdot \frac{du}{u} = \int_1^e e^{u - \ln u} \cdot \frac{du}{u} = \int_1^e e^{u - \ln u} \cdot \frac{du}{u} = \int_1^e e^{u - \ln u} \cdot \frac{du}{u} = \int_1^e e^{u - \ln u} \cdot \frac{du}{u} = \int_1^e e^{u - \ln u} \cdot \frac{du}{u} = \int_1^e e^{u - \ln u} \cdot \frac{du}{u} = \int_1^e e^{u - \ln u} \cdot \frac{du}{u} = \int_1^e e^{u - \ln u} \cdot \frac{du}{u} = \int_1^e e^{u - \ln u} \cdot \frac{du}{u} = \int_1^e e^{u - \ln u} \cdot \frac{du}{u} = \int_1^e e^{u - \ln u} \cdot \frac{du}{u} = \int_1^e e^{u - \ln u} \cdot \frac{du}{u} = \int_1^e e^{u - \ln u} \cdot \frac{du}{u} = \int_1^e e^{u - \ln u} \cdot \frac{du}{u} = \int_1^e e^{u - \ln u} \cdot \frac{du}{u} = \int_1^e e^{u - \ln u} \cdot \frac{du}{u} = \int_1^e e^{u - \ln u} \cdot \frac{du}{u} = \int_1^e e^{u - \ln u} \cdot \frac{du}{u} = \int_1^e e^{u - \ln u} \cdot \frac{du}{u} = \int_1^e e^{u - \ln u} \cdot \frac{du}{u} = \int_1^e e^{u - \ln u} \cdot \frac{du}{u} = \int_1^e e^{u - \ln u} \cdot \frac{du}{u} = \int_1^e e^{u - \ln u} \cdot \frac{du}{u} = \int_1^e e^{u - \ln u} \cdot \frac{du}{u} = \int_1^e e^{u - \ln u} \cdot \frac{du}{u} = \int_1^e e^{u - \ln u} \cdot \frac{du}{u} = \int_1^e e^{u - \ln u} \cdot \frac{du}{u} = \int_1^e e^{u - \ln u} \cdot \frac{du}{u} = \int_1^e e^{u - \ln u} \cdot \frac{du}{u} = \int_1^e e^{u - \ln u} \cdot \frac{du}{u} = \int_1^e e^{u - \ln u} \cdot \frac{du}{u} = \int_1^e e^{u - \ln u} \cdot \frac{du}{u} = \int_1^e e^{u - \ln u} \cdot \frac{du}{u} = \int_1^e e^{u - \ln u} \cdot \frac{du}{u} = \int_1^e e^{u - \ln u} \cdot \frac{du}{u} = \int_1^e e^{u - \ln u} \cdot \frac{du}{u} = \int_1^e e^{u - \ln u} \cdot \frac{du}{u} = \int_1^e e^{u - \ln u} \cdot \frac{du}{u} = \int_1^e e^{u - \ln u} \cdot \frac{du}{u} = \int_1^e e^{u - \ln u} \cdot \frac{du}{u} = \int_1^e e^{u - \ln u} \cdot \frac{du}{u} = \int_1^e e^{u - \ln u} \cdot \frac{du}{u} = \int_1^e e^{u - \ln u} \cdot \frac{du}{u} = \int_1^e e^{u - \ln u} \cdot \frac{du}{u} = \int_1^e e^{u - \ln u} \cdot \frac{du}{u} = \int_1^e e^{u - \ln u} \cdot \frac{du}{u} = \int_1^e e^{u - \ln u} \cdot \frac{du}{u} = \int_1^e e^{u - \ln u} \cdot \frac{du}{u} = \int_1^e e^{u - \ln u} \cdot \frac{du}{u} = \int_1^e e^{u - \ln u} \cdot \frac{du}{u} = \int_1^e e^{u - \ln u} \cdot \frac{du}{u} = \int_1^e e^{u - \ln u} \cdot \frac{du}{u} = \int_1^e e^{u - \ln u} \cdot \frac{du}{u} = \int_1^e e^{u - \ln u} \cdot \frac{du}{u} = \int_1^e e^{u - \ln u} \cdot \frac{du}{u} = \int_1^e e^{u - \ln u} \cdot \frac{du}{u} = \int_1^e e^{u - \ln u} \cdot \frac{du}{u} = \int_1^e e^{u - \ln u} \cdot \frac{du}{u} = \int_1^e e^{u - \ln u} \cdot \frac{du}{u} = \int_1^e e^{u - \ln u} \cdot \frac{du}{u} = \int_1^e e^{u - \ln u} \cdot \frac{du}{u} = \int_1^e e^{u - \ln u} \cdot \frac{du}{u} = \int_1^e e^{u - \ln u} \cdot \frac{du}{u} = \int_1^e e^{u - \ln u} \cdot \frac{du}{u} = \int_1^e e^{u - \ln u} \cdot \frac{du}{u} = \int_1^e e^{u - \ln u} \cdot \frac{du}{u} = \int_1^e e^{u - \ln u} \cdot \frac{du}{u} = \int_1^e e^{u - \ln u} \cdot \frac{du}{u} = \int_1^e e^{u - \ln u} \cdot \frac{du}{u} = \int_1^e e^{u - \ln u} \cdot \frac{du}{u} = \int_1^e e^{u - \ln u} \cdot \frac{du}{u} = \int_1^e e^{u - \ln u} \cdot \frac{du}{u} = \int_1^e e^{u - \ln u} \cdot \frac{du}{u} = \int_1^e e^{u - \ln u} \cdot \frac{du}{u} = \int_1^e e^{u - \ln u} \cdot \frac{du}{u} = \int_1^e e^{u - \ln u} \cdot \frac{du}{u} = \int_1^e e^{u - \ln u} \cdot \frac{du}{u} = \int_1^e e^{u - \ln u} \cdot \frac{du}{u} = \int_1^e e^{u - \ln u} \cdot \frac{du}{u} = \int_1^e e^{u - \ln u} \cdot \frac{du}{u} = \int_1^e e^{u - \ln u} \cdot \frac{du}{u} = \int_1^e e^{u - \ln u} \cdot \frac{du}{u} = \int_1^e e^{u - \ln u} \cdot \frac{du}{u} = \int_1^e e^{u - \ln u} \cdot \frac{du}{u} = \int_1^e e^{u - \ln u} \cdot \frac{du}{u} = \int_1^e e^{u - \ln u} \cdot \frac{du}{u} = \int_1^e e^{u - \ln u} \cdot \frac{du}{u} = \int_1^e e^{u - \ln u} \cdot \frac{du}{u} = \int_1^e e^{u - \ln u} \cdot \frac{du}{u} = \int_1^e e^{u - \ln u} \cdot \frac{du}{u} = \int_1^e e^{u - \ln u} \cdot \frac{du}{u} = \int_1^e e^{u - \ln u} \cdot \frac{du}{u} = \int_1^e e^{u - \ln u} \cdot \frac{du}{u} = \int_1^e e^{u - \ln u} \cdot \frac{du}{u} = \int_1^e e^{u - \ln u} \cdot \frac{du}{u} = \int_1^e e^{u - \ln u} \cdot \frac{du}{u} = \int_1^e e^{u - \ln u} \cdot \frac{du}{u} = \int_1^e e^{u - \ln u} \cdot \frac{du}{u} = \int_1^e e^{u - \ln u} \cdot \frac{du}{u} = \int_1^e e^{u - \ln u} \cdot \frac{du}{u} = \int_1^e e^{u - \ln u} \cdot \frac{du}{u} = \int_1^e e^{u - \ln u} \cdot \frac{du}{u} = \int_1^e e^{u - \ln u} \cdot \frac{du}{u} = \int_1^e e^{u - \ln u} \cdot \frac{du}{u} = \int_1^e e^{u - \ln u} \cdot \frac{du}{u} = \int_1^e e^{u - \ln u} \cdot \frac{du}{u} = \int_1^e e^{u - \ln u} \cdot \frac{du}{u} = \int_1^e e^{u - \ln u} \cdot \frac{du}{u} = \int_1^e e^{u - \ln u} \cdot \frac{du}{u} = \int_1^e e^{u - \ln u} \cdot \frac{du}{u} = \int_1^e e^{u - \ln u} \cdot \frac{du}{u} = \int_1^e e^{u - \ln u} \cdot \frac{du}{u} = \int_1^e e^{u - \ln u} \cdot \frac{du}{u} = \int_1^e e^{u - \ln u} \cdot \frac{du}{u} = \int_1^e e^{u - \ln u} \cdot \frac{du}{u} = \int_1^e e^{u - \ln u} \cdot \frac{du}{u} = \int_1^e e^{u - \ln u} \cdot \frac{du}{u} = \int_1^e e^{u - \ln u} \cdot \frac{du}{u} = \int_1^e e^{u - \ln u} \cdot \frac{du}{u} = \int_1^e e^{u - \ln u} \cdot \frac{du}{u} = \int_1^e e^{u - \ln u} \cdot \frac{du}{u} = \int_1^e e^{u - \ln u} \cdot \frac{du}{u} = \int_1^e e^{u - \ln u} \cdot \frac{du}{u} = \int_1^e e^{u - \ln u} \cdot \frac{du}{u} = \int_1^e e^{u - \ln u} \cdot \frac{du}{u} = \int_1^e e^{u - \ln u} \cdot \frac{du}{u} = \int_1^e e^{u - \ln u} \cdot \frac{du}{u} = \int_1^e e^{u - \ln u} \cdot \frac{du}{u} = \int_1^e e^{u - \ln u} \cdot \frac{du}{u} = \int_1^e e^{u - \ln u} \cdot \frac{du}{u} = \int_1^e e^{u - \ln u} \cdot \frac{du}{u} = \int_1^e e^{u - \ln u} \cdot \frac{du}{u} = \int_1^e e^{u - \ln u} \cdot \frac{du}{u} = \int_1^e e^{u - \ln u} \cdot \frac{du}{u} = \int_1^e e^{u - \ln u} \cdot \frac{du}{u} = \int_1^e e^{u - \ln u} \cdot \frac{du}{u} = \int_1^e e^{u - \ln u} \cdot \frac{du}{u} = \int_1^e e^{u - \ln u} \cdot \frac{du}{u} = \int_1^e e^{u - \ln u} \cdot \frac{du}{u} = \int_1^e e^{u - \ln u} \cdot \frac{du}{u} = \int_1^e e^{u - \ln u} \cdot \frac{du}{u} = \int_1^e e^{u - \ln u} \cdot \frac{du}{u} = \int_1^e e^{u - \ln u} \cdot \frac{du}{u} = \int_1^e e^{u - \ln u} \cdot \frac{du}{u} = \int_1^e e^{u - \ln u} \cdot \frac{du}{u} = \int_1^e e^{u - \ln u} \cdot \frac{du}{u} = \int_1^e e^{u - \ln u} \cdot \frac{du}{u} = \int_1^e e^{u - \ln u} \cdot \frac{du}{u} = \int_1^e e^{u - \ln u} \cdot \frac{du}{u} = \int_1^e e^{u - \ln u} \cdot \frac{du}{u} = \int_1^e e^{u - \ln u} \cdot \frac{du}{u} = \int_1^e e^{u - \ln u} \cdot \frac{du}{u} = \int_1^e e^{u - \ln u} \cdot \frac{du}{u} = \int_1^e e^{u - \ln u} \cdot \frac{du}{u} = \int_1^e e^{u - \ln u} \cdot \frac{du}{u} = \int_1^e e^{u - \ln u} \cdot \frac{du}{u} = \int_1^e e^{u - \ln u} \cdot \frac{du}{u} = \int_1^e e^{u - \ln u} \cdot \frac{du}{u} = \int_1^e e^{u - \ln u} \cdot \frac{du}{u} = \int_1^e e^{u - \ln u} \cdot \frac{du}{u} = \int_1^e e^{u - \ln u} \cdot \frac{du}{u} = \int_1^e e^{u - \ln u} \cdot \frac{du}{u} = \int_1^e e^{u - \ln u} \cdot \frac{du}{u} = \int_1^e e^{u - \ln u} \cdot \frac{du}{u} = \int_1^e e^{u - \ln u} \cdot \frac{du}{u} = \int_1^e e^{u - \ln u} \cdot \frac{du}{u} = \int_1^e e^{u - \ln u} \cdot \frac{du}{u} = \int_1^e e^{u - \ln u} \cdot \frac{du}{u} = \int_1^e e^{u - \ln u} \cdot \frac{du}{u} = \int_1^e e^{u - \ln u} \cdot \frac{du}{u} = \int_1^e e^{u - \ln u} \cdot \frac{du}{u} = \int_1^e e^{u - \ln u} \cdot \frac{du}{u} = \int_1^e e^{u - \ln u} \cdot \frac{du}{u} = \int_1^e e^{u - \ln u} \cdot \frac{du}{u} = \int_1^e e^{u - \ln u} \cdot \frac{du}{u} = \int_1^e e^{u - \ln u} \cdot \frac{du}{u} = \int_1^e e^{u - \ln u} \cdot \frac{du}{u} = \int_1^e e^{u - \ln u} \cdot \frac{du}{u} = \int_1^e e^{u - \ln u} \cdot \frac{du}{u} = \int_1^e e^{u - \ln u} \cdot \frac{du}{u} = \int_1^e e^{u - \ln u} \cdot \frac{du}{u} = \int_1^e e^{u - \ln u} \cdot \frac{du}{u} = \int_1^e e^{u - \ln u} \cdot \frac{du}{u} = \int_1^e e^{u - \ln u} \cdot \frac{du}{u} = \int_1^e e^{u - \ln u} \cdot \frac{du}{u} = \int_1^e e^{u - \ln u} \cdot \frac{du}{u} = \int_1^e e^{u - \ln u} \cdot \frac{du}{u} = \int_1^e e^{u - \ln u} \cdot \frac{du}{u} = \int_1^e e^{u - \ln u} \cdot \frac{du}{u} = \int_1^e e^{u - \ln u} \cdot \frac{du}{u} = \int_1^e e^{u - \ln u} \cdot \frac{du}{u} = \int_1^e e^{u - \ln u} \cdot \frac{du}{u} = \int_1^e e^{u - \ln u} \cdot \frac{du}{u} = \int_1^e e^{u - \ln u} \cdot \frac{du}{u} = \int_1^e e^{u - \ln u} \cdot \frac{du}{u} = \int_1^e e^{u - \ln u} \cdot \frac{du}{u} = \int_1^e e^{u - \ln u} \cdot \frac{du}{u} = \int_1^e e^{u - \ln u} \cdot \frac{du}{u} = \int_1^e e^{u - \ln u} \cdot \frac{du}{u} = \int_1^e e^{u - \ln u} \cdot \frac{du}{u} = \int_1^e e^{u - \ln u} \cdot \frac{du}{u} = \int_1^e e^{u - \ln u} \cdot \frac{du