<think>
Okay, let's tackle this integral: ∫₀¹ x^(1/2) [1 - √(x(1-x))]^(-2) dx. Hmm, first, I need to simplify the integrand if possible. Let me write it out again: x^(1/2) divided by [1 - √(x(1-x))]^2. Wait, the denominator is [1 - √(x(1 - x))] squared. Maybe simplifying the expression inside the square root first. Let's see, x(1 - x) is a quadratic expression, which might relate to a trigonometric substitution or maybe a beta function?

Alternatively, let's consider substitution. Let me set t = √x. Then x = t², dx = 2t dt. When x=0, t=0; x=1, t=1. So the integral becomes ∫₀¹ t [1 - √(t²(1 - t²))]^(-2) * 2t dt. Simplify inside the square root: √(t²(1 - t²)) = t√(1 - t²). So the denominator becomes [1 - t√(1 - t²)]². Then the integral is 2 ∫₀¹ t² / [1 - t√(1 - t²)]² dt. Hmm, not sure if that's better. Maybe another substitution?

Alternatively, let's look at the denominator: 1 - √(x(1 - x)). Let me denote u = √x. Then x = u², dx = 2u du. Then the integral becomes ∫₀¹ u [1 - u√(1 - u²)]^(-2) * 2u du = 2 ∫₀¹ u² / [1 - u√(1 - u²)]² du. Still similar to the previous substitution. Maybe another approach.

Wait, maybe rationalizing the denominator? Let's see. The denominator is [1 - √(x(1 - x))]^2. Let's expand that. Let me compute 1 - √(x(1 - x)) first. Let me call the term inside the square root as y = x(1 - x). Then denominator is (1 - √y)^2 = 1 - 2√y + y. So the integrand becomes x^(1/2) / (1 - 2√(x(1 - x)) + x(1 - x)). Hmm, not sure if that helps. Maybe expanding the denominator?

Alternatively, perhaps a substitution to make the integral look like a standard form. Let me consider trigonometric substitution. Let’s set x = sin²θ. Then dx = 2 sinθ cosθ dθ. When x=0, θ=0; x=1, θ=π/2. Let's substitute. The integrand becomes [sin²θ]^(1/2) / [1 - √(sin²θ (1 - sin²θ))]^2 * 2 sinθ cosθ dθ. Simplify: sinθ / [1 - √(sin²θ cos²θ)]² * 2 sinθ cosθ dθ. The square root term is sinθ cosθ, so denominator becomes [1 - sinθ cosθ]^2. So the integral becomes 2 ∫₀^(π/2) [sinθ * sinθ cosθ] / [1 - sinθ cosθ]^2 dθ. Simplify numerator: 2 sin²θ cosθ. So integral is 2 ∫ sin²θ cosθ / (1 - sinθ cosθ)^2 dθ. Hmm, not sure if that's better. Let me check the substitution again. Wait, maybe there's a mistake here. Let me re-express the denominator. Wait, when x = sin²θ, then 1 - x = cos²θ, so x(1 - x) = sin²θ cos²θ, so √( x(1 - x) ) = sinθ cosθ. So denominator is (1 - sinθ cosθ)^2. The numerator is x^(1/2) dx = sinθ * 2 sinθ cosθ dθ. So numerator is 2 sin²θ cosθ dθ. So the integral becomes 2 ∫₀^(π/2) [sin²θ cosθ] / (1 - sinθ cosθ)^2 dθ. Hmm, maybe this is helpful. Let me see if I can manipulate this.

Let me denote t = sinθ cosθ. Wait, but integrating in terms of θ. Alternatively, perhaps use substitution u = 1 - sinθ cosθ. Let me try that. Let u = 1 - sinθ cosθ. Then du/dθ = - [cos²θ - sin²θ] = -cos(2θ). Hmm, not sure. Alternatively, maybe express sinθ cosθ as (1/2) sin(2θ). So denominator becomes [1 - (1/2) sin2θ]^2. Then the integral is 2 ∫₀^(π/2) [sin²θ cosθ] / [1 - (1/2) sin2θ]^2 dθ. Hmm, not sure. Maybe expand the denominator as a series? But that might complicate things. Alternatively, perhaps another substitution.

Wait, let's consider the integral in terms of t = sinθ. Then θ = arcsin t, dθ = dt / √(1 - t²). But when θ goes from 0 to π/2, t goes from 0 to 1. Let's see. Then sinθ = t, cosθ = √(1 - t²). Then sinθ cosθ = t√(1 - t²). The integral becomes 2 ∫₀¹ [t² * √(1 - t²)] / [1 - t√(1 - t²)]² * [dt / √(1 - t²)]}. Wait, that seems messy. Let me check again. Wait, original integral after substitution is 2 ∫ sin²θ cosθ / (1 - sinθ cosθ)^2 dθ. If t = sinθ, then cosθ dθ = dt. So sin²θ cosθ dθ = t² dt. Then the integral becomes 2 ∫₀¹ t² / (1 - t√(1 - t²))² dt. Wait, that's the same as the substitution we did earlier with t = √x. So maybe this isn't helpful. Hmm.

Alternatively, perhaps rationalize the denominator. Let me consider multiplying numerator and denominator by [1 + √(x(1 - x))]^2. Then denominator becomes [1 - x(1 - x)]^2. Wait, because (a - b)(a + b) = a² - b². So [1 - √(x(1 - x))]^2 * [1 + √(x(1 - x))]^2 = [1 - x(1 - x)]². So the integrand becomes x^(1/2) [1 + √(x(1 - x))]^2 / [1 - x(1 - x)]². Let me compute 1 - x(1 - x) = 1 - x + x². So denominator is (1 - x + x²)^2. The numerator is x^(1/2) [1 + √(x(1 - x))]^2. Let's expand the numerator: [1 + 2√(x(1 - x)) + x(1 - x)]. So the integrand becomes x^(1/2) [1 + 2√(x(1 - x)) + x(1 - x)] / (1 - x + x²)^2. Hmm, not sure if that's better, but maybe splitting into terms.

So split the integrand into three parts:

1. x^(1/2) / (1 - x + x²)^2

2. 2 x^(1/2) √(x(1 - x)) / (1 - x + x²)^2

3. x^(1/2) * x(1 - x) / (1 - x + x²)^2

Simplify each term:

First term: x^(1/2) / (1 - x + x²)^2

Second term: 2 x^(1/2) * x^(1/2) (1 - x)^(1/2) / (1 - x + x²)^2 = 2 x (1 - x)^(1/2) / (1 - x + x²)^2

Third term: x^(3/2) (1 - x) / (1 - x + x²)^2

Hmm, not sure if this helps. Maybe integrating term by term? But these still look complicated. Let me check if substitution can be applied here. For example, substitution for 1 - x + x². Let me set u = x - 1/2, which might make the quadratic symmetric. Then x = u + 1/2, dx = du. Then 1 - x + x² = 1 - (u + 1/2) + (u + 1/2)^2 = 1 - u - 1/2 + u² + u + 1/4 = 1 - 1/2 + 1/4 + u² + ( -u + u ) = 3/4 + u². So 1 - x + x² = u² + 3/4. Hmm, that's a standard quadratic. So maybe substitution for the first term. Let's see:

First term: x^(1/2) / (u² + 3/4)^2. But x = u + 1/2, so x^(1/2) = sqrt(u + 1/2). Hmm, not sure. Maybe this substitution isn't helpful. Alternatively, perhaps use partial fractions? But the denominator is (1 - x + x²)^2, which is irreducible over real numbers. So partial fractions might not be straightforward.

Alternatively, maybe consider integrating in the complex plane, but that's probably overkill. Let me think of another approach. Maybe substitution using hypergeometric functions? Not sure. Alternatively, check if the integral can be expressed in terms of known constants or beta functions. Wait, the original integral is from 0 to 1, which is a common interval for beta functions. The beta function is ∫₀¹ t^{c-1} (1 - t)^{d-1} dt. But our integrand is more complicated. Let me see.

Alternatively, maybe substitution t = √x. Wait, tried that earlier. Let me try again. Let t = x^{1/2}, so x = t², dx = 2t dt. Then the integral becomes ∫₀¹ t [1 - t√(1 - t²)]^{-2} * 2t dt = 2 ∫₀¹ t² / [1 - t√(1 - t²)]² dt. Let me denote u = t√(1 - t²). Then maybe express in terms of u. But differentiating u: du/dt = √(1 - t²) + t*( - t / √(1 - t²) ) = √(1 - t²) - t² / √(1 - t²) = (1 - t² - t²)/√(1 - t²) = (1 - 2t²)/√(1 - t²). Hmm, not sure if that helps. Maybe not helpful.

Alternatively, let's consider substitution v = t². Then t = sqrt(v), dt = (1/(2√v)) dv. But not sure. Alternatively, maybe substitution to rationalize the denominator. Let me set s = t√(1 - t²). Then s = t√(1 - t²). Let me square both sides: s² = t²(1 - t²). So s² = t² - t⁴. Rearranged: t⁴ - t² + s² = 0. Hmm, this seems complicated. Maybe not helpful.

Alternatively, let's consider a substitution where we set z = t². Then t = sqrt(z), dt = (1/(2√z)) dz. Then the integral becomes 2 ∫₀¹ z / [1 - sqrt(z) sqrt(1 - z)]² * (1/(2√z)) dz = ∫₀¹ sqrt(z) / [1 - sqrt(z(1 - z))]² dz. Wait, that's the same as the original integral. Hmm, going in circles.

Wait, maybe try numerical methods? But the problem says to compute it analytically first. So perhaps there's a trick I'm missing. Let me think again at the original integrand: x^{1/2} / [1 - sqrt(x(1 - x))]^2. Let me consider expanding the denominator as a power series. Let me denote y = sqrt(x(1 - x)). Then the denominator is (1 - y)^2. So 1/(1 - y)^2 = Σ_{n=1}^∞ n y^{n-1} }, but wait, the expansion of 1/(1 - y)^2 is Σ_{n=0}^\infty (n + 1) y^n. So maybe expand the integrand as a power series in y, then integrate term by term.

So, 1/(1 - y)^2 = Σ_{n=0}^\infty (n + 1) y^n. Therefore, the integrand becomes x^{1/2} * Σ_{n=0}^\infty (n + 1) y^n = Σ_{n=0}^\infty (n + 1) x^{1/2} [x(1 - x)]^{n/2}. Simplify [x(1 - x)]^{n/2} = x^{n/2} (1 - x)^{n/2}. So the integrand becomes Σ_{n=0}^\infty (n + 1) x^{(1 + n)/2} (1 - x)^{n/2}. Then the integral becomes Σ_{n=0}^\infty (n + 1) ∫₀¹ x^{(1 + n)/2} (1 - x)^{n/2} dx. This integral is a beta function. The integral ∫₀¹ x^{a} (1 - x)^b dx = B(a+1, b+1) = Γ(a+1)Γ(b+1)/Γ(a + b + 2). Here, a = (1 + n)/2, b = n/2. So the integral becomes B((1 + n)/2 + 1, n/2 + 1) = B((n + 3)/2, (n + 2)/2). Then Γ((n + 3)/2)Γ((n + 2)/2) / Γ(n + 5/2 + 1/2) = Γ((n + 3)/2)Γ((n + 2)/2) / Γ(n + 3). Hmm, but Γ(n + 3) = (n + 2)!.

But Γ((n + 3)/2) and Γ((n + 2)/2) can be expressed using the duplication formula or properties of the gamma function. Let me recall that Γ(z)Γ(z + 1/2) = 2^{1 - 2z} √π Γ(2z). Let me check if that applies here. Let’s = (n + 2)/2 and (n + 3)/2. The product Γ((n + 2)/2)Γ((n + 3)/2) = Γ(z)Γ(z + 1/2) where z = (n + 2)/2. So applying the duplication formula: Γ(z)Γ(z + 1/2) = 2^{1 - 2z} √π Γ(2z). So here, 2z = n + 2. Therefore, Γ(z)Γ(z + 1/2) = 2^{1 - (n + 2)} √π Γ(n + 2). So 2^{-n -1} √π (n + 1)!.

Therefore, the beta function B((n + 3)/2, (n + 2)/2) = [2^{-n -1} √π (n + 1)! ] / Γ(n + 3). But Γ(n + 3) = (n + 2)! So this becomes [2^{-n -1} √π (n + 1)! ] / (n + 2)! ) = 2^{-n -1} √π / (n + 2). Therefore, the integral becomes Σ_{n=0}^\infty (n + 1) * [2^{-n -1} √π / (n + 2)].

Simplify the sum: Σ_{n=0}^\infty (n + 1) * 2^{-n -1} √π / (n + 2). Let’s factor out √π / 2: (√π / 2) Σ_{n=0}^\infty (n + 1) / (2^n (n + 2)). Let’s make substitution k = n + 2. Then n = k - 2, but when n=0, k=2. So the sum becomes Σ_{k=2}^\infty (k - 1) / (2^{k - 2} k). Hmm, not sure. Alternatively, let's write (n + 1)/(n + 2) = 1 - 1/(n + 2). So the sum becomes Σ_{n=0}^\infty [1 - 1/(n + 2)] * 2^{-n -1} √π. Then split into two sums: √π / 2 [ Σ_{n=0}^\infty 2^{-n} - Σ_{n=0}^\infty 2^{-n}/(n + 2) ) ].

First sum: Σ_{n=0}^\infty 2^{-n} = 1 / (1 - 1/2) = 2. Second sum: Σ_{n=0}^\infty 2^{-n}/(n + 2). Let’s adjust index for the second sum. Let m = n + 2, so n = m - 2. When n=0, m=2. So Σ_{m=2}^\infty 2^{-(m - 2)} / m = 2^2 Σ_{m=2}^\infty 2^{-m} / m = 4 Σ_{m=2}^\infty (1/2^m)/m. But Σ_{m=1}^\infty (1/2^m)/m = -ln(1 - 1/2) = ln 2. So Σ_{m=2}^\infty (1/2^m)/m = ln 2 - (1/2)/1 = ln 2 - 1/2. Therefore, the second sum is 4 (ln 2 - 1/2). Therefore, the total sum is √π / 2 [ 2 - 4 (ln 2 - 1/2) ] = √π / 2 [ 2 - 4 ln 2 + 2 ] = √π / 2 [4 - 4 ln 2] = √π / 2 * 4 (1 - ln 2) = 2 √π (1 - ln 2). Wait, let me check the steps again.

Wait, first sum: √π / 2 multiplied by [ Σ 2^{-n} ] which is 2, so √π / 2 * 2 = √π. Then subtract √π / 2 multiplied by the second sum, which is 4 (ln 2 - 1/2). So total is √π - √π / 2 * 4 (ln 2 - 1/2) = √π - 2√π (ln 2 - 1/2) = √π [1 - 2 ln 2 + 1] = √π (2 - 2 ln 2) = 2√π (1 - ln 2). Wait, but let me verify the second sum again. The original second sum is Σ_{n=0}^\infty 2^{-n}/(n + 2). Let me compute that. Let’s write it as Σ_{n=0}^\infty 2^{-n}/(n + 2) = Σ_{k=2}^\infty 2^{-(k - 2)}/k = 4 Σ_{k=2}^\infty 2^{-k}/k. Then Σ_{k=1}^\infty 2^{-k}/k = -ln(1 - 1/2) = ln 2. So Σ_{k=2}^\infty 2^{-k}/k = ln 2 - 2^{-1}/1 = ln 2 - 1/2. Therefore, the second sum is 4 (ln 2 - 1/2). So the total expression is √π / 2 [2 - 4(ln 2 - 1/2)] = √π / 2 [2 - 4 ln 2 + 2] = √π / 2 (4 - 4 ln 2) = √π * 2 (1 - ln 2). So the integral equals 2√π (1 - ln 2). Wait, that seems plausible. Let me check the steps again.

Original integral after expansion: Σ_{n=0}^\infty (n + 1) * [2^{-n -1} √π / (n + 2)].

So that's (√π / 2) Σ_{n=0}^\infty (n + 1)/(n + 2) * 2^{-n}.

Then (n + 1)/(n + 2) = 1 - 1/(n + 2). So split into two sums:

(√π / 2) [ Σ_{n=0}^\infty 2^{-n} - Σ_{n=0}^\infty 2^{-n}/(n + 2) ].

First sum is Σ 2^{-n} = 2. Second sum is Σ_{n=0}^\infty 2^{-n}/(n + 2) = 4 Σ_{k=2}^\infty 2^{-k}/k = 4 (ln 2 - 1/2). So the total is (√π / 2)(2 - 4(ln 2 - 1/2)) = (√π / 2)(2 - 4 ln 2 + 2) = (√π / 2)(4 - 4 ln 2) = 2√π (1 - ln 2). Therefore, the integral equals 2√π (1 - ln 2). Wait, but ln 2 is natural logarithm of 2. So the exact answer is 2√π (1 - ln 2). Let me check if this makes sense dimensionally. The integral is over [0,1], and the integrand is positive, so the result should be positive. Since ln 2 ≈ 0.6931, 1 - ln 2 ≈ 0.3069, so 2√π * 0.3069 ≈ 2 * 1.77245 * 0.3069 ≈ 1.77245 * 0.6138 ≈ 1.088. Let me check numerically later.

But let me verify if the steps are correct. The expansion of 1/(1 - y)^2 as a power series is correct. Then term-by-term integration, assuming convergence, which should be valid here since y = sqrt(x(1 - x)) is between 0 and 1/2 for x in [0,1], so the series converges. Then the use of beta function and gamma functions, applying the duplication formula. Then simplifying the sum. The key step was splitting (n + 1)/(n + 2) into 1 - 1/(n + 2), which allows expressing the sum in terms of known series. Then using the fact that Σ_{k=1}^\infty (1/2^k)/k = ln 2. Therefore, the steps seem correct.

Therefore, the exact answer is 2√π (1 - ln 2). Let me write that in LaTeX: 2\sqrt{\pi}(1 - \ln 2). Now, compute the numerical approximation. Let's calculate:

√π ≈ 1.7724538509

ln 2 ≈ 0.69314718056

So 1 - ln 2 ≈ 1 - 0.69314718056 ≈ 0.30685281944

Multiply by 2√π: 2 * 1.7724538509 * 0.30685281944 ≈

First, 2 * 1.7724538509 ≈ 3.5449077018

Then 3.5449077018 * 0.30685281944 ≈

Let me compute 3.5449077018 * 0.3 = 1.06347231054

3.5449077018 * 0.00685281944 ≈

0.00685281944 * 3.5449077018 ≈

Approximately: 0.006 * 3.5449 ≈ 0.0212694, 0.00085281944 * 3.5449 ≈ 0.003025

Total ≈ 0.0212694 + 0.003025 ≈ 0.0242944

So total ≈ 1.06347231054 + 0.0242944 ≈ 1.0877667

Rounded to 10 decimal places: 1.0877667105. Let me use a calculator for more precision.

Alternatively, compute 3.5449077018 * 0.30685281944:

3.5449077018 × 0.30685281944

First, multiply 3.5449077018 × 0.3 = 1.06347231054

3.5449077018 × 0.00685281944:

Breakdown:

3.5449077018 × 0.006 = 0.02126944621

3.5449077018 × 0.00085281944 ≈ 3.5449077018 × 0.0008 = 0.00283592616

3.5449077018 × 0.00005281944 ≈ 0.0001873

Total ≈ 0.00283592616 + 0.0001873 ≈ 0.003023226

So total for 0.00685281944 part: 0.02126944621 + 0.003023226 ≈ 0.024292672

Adding to the 1.06347231054 gives 1.06347231054 + 0.024292672 ≈ 1.08776498254. Rounded to 10 decimal places: 1.0877649825 ≈ 1.0877649825. So approximately 1.0877649825. Let me check with a calculator.

Alternatively, use exact values:

2 * sqrt(pi) * (1 - ln 2) ≈ 2 * 1.7724538509055159 * (1 - 0.6931471805599453) ≈

Compute 1 - 0.6931471805599453 = 0.3068528194400547

Multiply by 1.7724538509055159: 1.7724538509055159 * 0.3068528194400547 ≈

Let me compute this:

1.7724538509055159 × 0.3 = 0.5317361552716548

1.7724538509055159 × 0.0068528194400547 ≈

0.0068528194400547 × 1.7724538509055159 ≈

Approximate:

0.006 × 1.7724538509 = 0.0106347231

0.00085281944 × 1.7724538509 ≈ 0.001512

Total ≈ 0.0106347231 + 0.001512 ≈ 0.0121467231

So total ≈ 0.5317361552716548 + 0.0121467231 ≈ 0.54388287837

Multiply by 2: 0.54388287837 × 2 ≈ 1.08776575674

So approximately 1.0877657567, which rounds to 1.0877657567, so to 10 decimal places: 1.0877657567. But let me check with a calculator for more precision.

Alternatively, use a calculator:

2 * sqrt(pi) * (1 - ln(2)):

sqrt(pi) ≈ 1.772453850905516

1 - ln(2) ≈ 0.3068528194400547

Multiply them: 1.772453850905516 * 0.3068528194400547 ≈

Let me do this step by step:

1.772453850905516 * 0.3 = 0.5317361552716548

1.772453850905516 * 0.0068528194400547 ≈

Calculate 1.772453850905516 * 0.006 = 0.010634723105433096

1.772453850905516 * 0.0008528194400547 ≈

0.0008528194400547 * 1.772453850905516 ≈

0. 0.772453850905516 * 0.00085281944 ≈ 0.000658

So total for 0.00085281944 part: 1.772453850905516 * 0.00085281944 ≈ 0.001512

So total for 0.00685281944 part: 0.0106347231 + 0.001512 ≈ 0.0121467231

Total product: 0.5317361552716548 + 0.0121467231 ≈ 0.54388287837

Multiply by 2: 0.54388287837 * 2 ≈ 1.08776575674

So the numerical approximation is approximately 1.0877657567, which rounds to 1.0877657567. Rounded to 10 decimal places: 1.0877657567. So 1.0877657567.

But let me verify using numerical integration. Let's compute the integral numerically to check. Let me approximate the integral ∫₀¹ sqrt(x) / (1 - sqrt(x(1 - x)))^2 dx.

Let me use substitution x = t^2, so dx = 2t dt. Then the integral becomes 2 ∫₀¹ t^2 / (1 - t sqrt(1 - t^2))^2 dt. Let me compute this numerically. Alternatively, use numerical integration tools. But since I can't compute it here, I'll trust the analytical result. However, given that the series expansion led to 2√π(1 - ln2) ≈ 1.0877657567, and if I compute the integral numerically, I should get a similar value. Let's assume that the analytical steps are correct, so the exact answer is 2√π(1 - ln2), and the numerical value is approximately 1.0877657567.
</think>

{"answer": "2\\sqrt{\\pi}(1 - \\ln 2)", "numerical_answer": "1.0877657567"}