We start with the integral

  I = ∫₀^(2π) tan(cos(x)) dx.

Step 1. Split the integration interval into two parts:
  I = ∫₀^(π) tan(cos(x)) dx + ∫₍π₎^(2π) tan(cos(x)) dx.

Step 2. In the second integral, perform the substitution u = x - π so that when x = π, u = 0 and when x = 2π, u = π. Also, note that
  cos(x) = cos(u + π) = -cos(u).

Thus the second integral becomes:
  ∫₍π₎^(2π) tan(cos(x)) dx = ∫₀^(π) tan(–cos(u)) du.

Since tan is an odd function (i.e. tan(–θ) = –tan(θ)), we have:
  tan(–cos(u)) = –tan(cos(u)).

Therefore,
  ∫₍π₎^(2π) tan(cos(x)) dx = –∫₀^(π) tan(cos(u)) du.

Step 3. Combine the two parts:
  I = ∫₀^(π) tan(cos(x)) dx – ∫₀^(π) tan(cos(x)) dx = 0.

Step 4. Numerical approximation:
  Since the exact value is 0, the numerical approximation is 0.0000000000.

Thus, the final answer is:

{"answer": "$0$", "numerical_answer": "0.0000000000"}