<think>
Okay, let's tackle this integral: the definite integral from 0 to 2 of x times the third Hermite polynomial evaluated at the square root of x(2 - x) dx. Hmm, so the integral is ∫₀² x H₃(√(x(2−x))) dx. 

First, I need to recall what the Hermite polynomials are. The third Hermite polynomial H₃(y) is given by H₃(y) = 8y³ - 12y. Let me confirm that. Yes, the standard physicists' Hermite polynomials start with H₀(y) = 1, H₁(y) = 2y, H₂(y) = 4y² - 2, H₃(y) = 8y³ - 12y. So that's correct.

So substituting y = √(x(2 - x)) into H₃, we get H₃(√(x(2−x))) = 8[√(x(2−x))]³ - 12√(x(2−x)). Therefore, the integrand becomes x*(8[x(2−x)]^(3/2) - 12[x(x−2)]^(1/2)). Wait, but x(2 - x) is under the square root, so [x(2 - x)]^(3/2) is (x(2 - x))^(1.5), and similarly for the other term.

So the integral becomes 8∫₀² x [x(2 - x)]^(3/2) dx - 12∫₀² x [x(2 - x)]^(1/2) dx. Let me denote these two integrals as I₁ and I₂, so the total integral is 8I₁ - 12I₂.

Now, I need to compute I₁ and I₂. Let's start with I₁ = ∫₀² x [x(2 - x)]^(3/2) dx. Let me make a substitution to simplify this. The expression under the square root is x(2 - x), which is symmetric around x = 1. Maybe a substitution like t = x - 1 would help, but let's see. Alternatively, use a trigonometric substitution. Let me think.

Alternatively, note that x(2 - x) = 2x - x² = -(x² - 2x) = -(x² - 2x +1 -1) = -(x -1)^2 +1. So it's a quadratic with vertex at (1,1). So maybe substituting t = x -1. Let t = x -1, so x = t +1, and when x=0, t=-1; x=2, t=1. Then x(2 - x) = (t +1)(1 - t) = 1 - t². So that's a useful substitution. So substituting t = x -1, then dx = dt, and the integral becomes:

For I₁: ∫ from t=-1 to t=1 of (t +1) [1 - t²]^(3/2) dt. Similarly, I₂ would be ∫ from t=-1 to t=1 of (t +1) [1 - t²]^(1/2) dt.

That's a good simplification. So now, both integrals are over symmetric intervals. Let's handle I₁ first.

I₁ = ∫_{-1}^1 (t +1)(1 - t²)^(3/2) dt. Let's split this into two integrals: ∫_{-1}^1 t(1 - t²)^(3/2) dt + ∫_{-1}^1 (1 - t²)^(3/2) dt.

The first integral is ∫_{-1}^1 t(1 - t²)^(3/2) dt. The integrand is an odd function because t is odd and (1 - t²)^(3/2) is even. So the product is odd. The integral over symmetric limits of an odd function is zero. Therefore, the first term is zero. So I₁ reduces to ∫_{-1}^1 (1 - t²)^(3/2) dt.

Similarly, for I₂: ∫_{-1}^1 (t +1)(1 - t²)^(1/2) dt. Again, split into ∫_{-1}^1 t(1 - t²)^(1/2) dt + ∫_{-1}^1 (1 - t²)^(1/2) dt. The first integral here is also an odd function, so it's zero. Therefore, I₂ = ∫_{-1}^1 (1 - t²)^(1/2) dt.

So now, both I₁ and I₂ are integrals of (1 - t²)^(n/2) over [-1,1], where n is 3 for I₁ and 1 for I₂. These are standard Beta function integrals. Recall that ∫_{-1}^1 (1 - t²)^k dt = 2 ∫₀^1 (1 - t²)^k dt. Let me confirm that. Yes, since (1 - t²)^k is even, so integrating from -1 to 1 is twice the integral from 0 to 1.

So for I₁: ∫_{-1}^1 (1 - t²)^(3/2) dt = 2 ∫₀^1 (1 - t²)^(3/2) dt. Let me make substitution u = t², but perhaps better to use the Beta function. The integral ∫₀^1 t^{m} (1 - t²)^n dt can be expressed in terms of Beta functions. Let me recall that ∫₀^1 t^{c -1} (1 - t)^{d -1} dt = B(c, d) = Γ(c)Γ(d)/Γ(c + d). But here, the integral is ∫₀^1 (1 - t²)^(3/2) dt. Let me set u = t², then t = sqrt(u), dt = (1/(2√u)) du. Wait, but maybe another substitution. Let u = t, then when t is from 0 to1, u is same. Let me instead use substitution t = sinθ. Let t = sinθ, then dt = cosθ dθ, and when t=0, θ=0; t=1, θ=π/2. Then (1 - t²)^(3/2) = (cos²θ)^(3/2) = cos³θ. So the integral becomes ∫₀^{π/2} cos³θ * cosθ dθ = ∫₀^{π/2} cos^4θ dθ. Wait, no. Wait, the substitution gives:

∫₀^1 (1 - t²)^(3/2) dt = ∫₀^{π/2} cos³θ * cosθ dθ = ∫₀^{π/2} cos^4θ dθ. Because when t = sinθ, dt = cosθ dθ, and sqrt(1 - t²) = cosθ. Wait, but (1 - t²)^(3/2) is cos³θ, and dt is cosθ dθ, so the integral becomes ∫ cos³θ * cosθ dθ = ∫ cos^4θ dθ. Yes. Similarly, for the integral in I₂, which is ∫₀^1 (1 - t²)^(1/2) dt, substitution t = sinθ would give ∫₀^{π/2} cosθ * cosθ dθ = ∫ cos²θ dθ.

But these integrals can be evaluated using the Beta function. Alternatively, use the formula for ∫ cos^nθ} dθ. The integral of cos^4θ from 0 to π/2 is (3π)/16. Let me check that. The formula for ∫₀^{π/2} cos^nθ dθ is (sqrt(π)/2) Γ((n +1)/2)/Γ((n +2)/2). For n=4, it's (sqrt(π)/2) Γ(5/2)/Γ(3). Γ(5/2) = (3/2)(1/2)sqrt(π) = (3/4)sqrt(π). Γ(3) = 2! = 2. So the integral is (sqrt(π)/2) * (3/4 sqrt(π)) / 2 = (sqrt(π)/2) * (3 sqrt(π)/8) = (3 π)/16. Yes, that's correct. So ∫₀^{π/2} cos^4θ dθ = 3π/16. Therefore, I₁ = 2 * 3π/16 = 3π/8.

Similarly, for I₂: ∫_{-1}^1 (1 - t²)^(1/2) dt = 2 ∫₀^1 (1 - t²)^(1/2) dt. Using substitution t = sinθ, this becomes 2 ∫₀^{π/2} cosθ * cosθ dθ = 2 ∫₀^{π/2} cos²θ dθ. The integral of cos²θ from 0 to π/2 is π/4. So 2*(π/4) = π/2. Therefore, I₂ = π/2.

Wait, let me confirm that. ∫ cos²θ dθ from 0 to π/2. The formula for ∫ cos^nθ dθ when n=2 is (sqrt(π)/2) Γ(3/2)/Γ(2). Γ(3/2) = (1/2)sqrt(π), Γ(2) =1. So (sqrt(π)/2) * (1/2 sqrt(π)) / 1 = (π)/4. So yes, ∫₀^{π/2} cos²θ dθ = π/4. Therefore, I₂ = 2*(π/4) = π/2. Correct.

So now, going back to the original integrals. The total integral is 8I₁ -12I₂ = 8*(3π/8) -12*(π/2) = 3π -6π = -3π. Wait, that's interesting. So the exact answer is -3π. Let me check the steps again to make sure.

First, H₃(y) = 8y³ -12y. Then, substituting y = sqrt(x(2 -x)), so H₃(sqrt(x(2 -x))) = 8*(x(2 -x))^(3/2) -12*(x(2 -x))^(1/2). Then, the integral becomes ∫₀² x*[8(x(2 -x))^(3/2) -12(x(2 -x))^(1/2)] dx. So that's 8∫x(x(2 -x))^(3/2) dx -12∫x(x(2 -x))^(1/2) dx. Then, substitution t = x -1, leading to I₁ and I₂ as above. Then, I₁ = 3π/8, I₂ = π/2. Then 8*I₁ = 8*(3π/8) = 3π, and 12*I₂ =12*(π/2)=6π. So 3π -6π = -3π. So the exact answer is -3π. 

But let me check if there was a sign error. When we did the substitution t = x -1, x = t +1, and x(2 -x) = (t +1)(1 -t) =1 -t². So that's correct. Then, the integrand for I₁ is (t +1)(1 -t²)^(3/2). Then splitting into t*(1 -t²)^(3/2) + (1 -t²)^(3/2). The first term is odd, so integrates to zero. The second term is even, so 2 times the integral from 0 to1. Then, substitution t = sinθ, leading to ∫ cos^4θ dθ, which is 3π/16. Multiply by 2 gives 3π/8. So that's correct. Similarly for I₂, the integral becomes 2*(π/4) = π/2. So 8*(3π/8) is 3π, 12*(π/2) is 6π. So 3π -6π = -3π. So the exact answer is -3π. 

But wait, the integral from 0 to2 of x H₃(sqrt(x(2 -x))) dx equals -3π. That seems a bit counterintuitive because the integrand might have positive and negative parts. Let me check with a numerical approximation. Let's compute the integral numerically to see if it's approximately -9.42477796... which is -3π. Let's see. π is approximately 3.1415926535, so 3π is about 9.42477796, so -3π is approximately -9.42477796. Let me check with a numerical approximation.

Alternatively, perhaps I made a mistake in the substitution. Let me check the substitution again. Let me take the integral I₁: ∫₀² x [x(2 -x)]^(3/2) dx. After substitution t = x -1, x = t +1, dx = dt. The limits from x=0 to x=2 become t=-1 to t=1. Then, x(2 -x) = (t +1)(1 -t) =1 -t². So [x(2 -x)]^(3/2) = (1 -t²)^(3/2). Then, x = t +1. So the integrand becomes (t +1)(1 -t²)^(3/2). Then splitting into t*(1 -t²)^(3/2) + (1 -t²)^(3/2). The first term is odd, so integral over symmetric interval is zero. The second term is even, so 2*∫₀¹ (1 -t²)^(3/2) dt. Then substitution t = sinθ, dt = cosθ dθ. When t=0, θ=0; t=1, θ=π/2. So the integral becomes 2*∫₀^{π/2} (1 - sin²θ)^(3/2) * cosθ dθ. Wait, but (1 - sin²θ)^(3/2) is cos³θ. Then, multiplied by cosθ dθ gives cos^4θ dθ. So 2*∫₀^{π/2} cos^4θ dθ. Which is 2*(3π/16) = 3π/8. Correct. So I₁ =3π/8. Then 8*I₁ =3π. Similarly, I₂ is ∫₀² x [x(2 -x)]^(1/2) dx. After substitution, same steps, becomes ∫_{-1}^1 (t +1)(1 -t²)^(1/2) dt. Split into t*(1 -t²)^(1/2) (which is odd, so integral zero) and (1 -t²)^(1/2) which is even. So 2*∫₀¹ (1 -t²)^(1/2) dt. Which is 2*(π/4) = π/2. Then 12*I₂ =6π. So 3π -6π = -3π. So the exact answer is -3π. 

But wait, the integrand: x H₃(sqrt(x(2 -x))). Let's check if H₃ is an odd function here. H₃(y) =8y³ -12y. So if y is sqrt(x(2 -x)), which is always non-negative. So H₃(y) =8y³ -12y. So depending on y, this could be positive or negative. For example, when y=0, H₃(0) = -0. But sqrt(x(2 -x)) is zero at x=0 and x=2, and reaches maximum at x=1, where sqrt(1*1)=1. So y ranges from 0 to1. So H₃(1) =8*1 -12*1= -4. So at x=1, the integrand is 1*(-4) = -4. At x=0.5, y= sqrt(0.5*1.5)=sqrt(0.75)≈0.866. H₃(y)=8*(0.866)^3 -12*(0.866). Let's compute that: 8*(0.866)^3 ≈8*(0.6495)≈5.196, and 12*0.866≈10.392. So 5.196 -10.392≈-5.196. So integrand at x=0.5 is 0.5*(-5.196)≈-2.598. So the integrand is negative over the interval. So the integral being negative makes sense. So the exact answer is -3π. 

Now, the numerical approximation. Since π≈3.141592653589793, so -3π≈-9.42477796076938. Rounded to 10 decimal places, that's -9.4247779608. 

So the final answer should be {"answer": "-3\\pi", "numerical_answer": "-9.4247779608"}.
</think>

{"answer": "-3\\pi", "numerical_answer": "-9.4247779608"}