
To solve the definite integral \(\int_{0}^{2} x \cos\left(\sqrt{x(2 - x)}\right) \, dx\), we proceed as follows:

### Step 1: Simplify the Argument of the Cosine Function
First, rewrite the expression inside the square root:
\[
x(2 - x) = 2x - x^2 = 1 - (x - 1)^2
\]
Thus, \(\sqrt{x(2 - x)} = \sqrt{1 - (x - 1)^2}\).

### Step 2: Substitution to Center the Integral
Let \(t = x - 1\), so \(x = t + 1\) and \(dx = dt\). The limits of integration change from \(x = 0\) to \(t = -1\) and \(x = 2\) to \(t = 1\). The integral becomes:
\[
\int_{-1}^{1} (t + 1) \cos\left(\sqrt{1 - t^2}\right) \, dt
\]

### Step 3: Split the Integral
Split the integral into two parts:
\[
\int_{-1}^{1} t \cos\left(\sqrt{1 - t^2}\right) \, dt + \int_{-1}^{1} \cos\left(\sqrt{1 - t^2}\right) \, dt
\]

### Step 4: Evaluate the First Integral
The first integrand \(t \cos\left(\sqrt{1 - t^2}\right)\) is an odd function (since \(t\) is odd and \(\cos\left(\sqrt{1 - t^2}\right)\) is even). The integral of an odd function over a symmetric interval \([-a, a]\) is zero. Thus:
\[
\int_{-1}^{1} t \cos\left(\sqrt{1 - t^2}\right) \, dt = 0
\]

### Step 5: Evaluate the Second Integral
The second integral is \(\int_{-1}^{1} \cos\left(\sqrt{1 - t^2}\right) \, dt\). Using the substitution \(t = \sin\theta\) (so \(dt = \cos\theta \, d\theta\) and \(\sqrt{1 - t^2} = \cos\theta\)), the limits change from \(t = -1\) to \(\theta = -\pi/2\) and \(t = 1\) to \(\theta = \pi/2\). The integral becomes:
\[
\int_{-\pi/2}^{\pi/2} \cos(\cos\theta) \cos\theta \, d\theta
\]
Since the integrand is even, this simplifies to:
\[
2 \int_{0}^{\pi/2} \cos(\cos\theta) \cos\theta \, d\theta
\]

### Step 6: Relate to Bessel Functions
Using the integral representation of the Bessel function \(J_1(z)\) (the Bessel function of the first kind of order 1), we know:
\[
J_1(1) = \frac{1}{\pi} \int_{0}^{\pi} \cos(\cos\theta) \cos\theta \, d\theta
\]
Thus, \(\int_{0}^{\pi} \cos(\cos\theta) \cos\theta \, d\theta = \pi J_1(1)\). Since the integrand is symmetric around \(\theta = \pi/2\), we have:
\[
2 \int_{0}^{\pi/2} \cos(\cos\theta) \cos\theta \, d\theta = \pi J_1(1)
\]

### Step 7: Combine Results
The original integral simplifies to \(\pi J_1(1)\).

### Numerical Approximation
The Bessel function \(J_1(1) \approx 0.4400505857\). Thus:
\[
\pi J_1(1) \approx 3.1415926536 \times 0.4400505857 \approx 1.3823007675
\]

### Final Answer
The exact answer is \(\pi J_1(1)\), and the numerical approximation is approximately \(1.3823007675\).

{"answer": "\(\pi J_1(1)\)", "numerical_answer": "1.3823007675"}