# Evaluating $\int\limits_{0}^{1}\ln\frac{1+0.5\sqrt{x}}{1-0.5\sqrt{x}}\:\mathrm{K}\left(\sqrt{1-x}\right)dx$

In this integral, $\mathrm{K}(k)$ represents the complete elliptic integral of the first kind.

## Step 1: Substitution

Let's make a substitution $t = \sqrt{x}$, which gives $x = t^2$ and $dx = 2t\,dt$. Also, $\sqrt{1-x} = \sqrt{1-t^2}$.

The integral becomes:
$$\int\limits_{0}^{1}\ln\frac{1+0.5\sqrt{x}}{1-0.5\sqrt{x}}\:\mathrm{K}\left(\sqrt{1-x}\right)dx = \int\limits_{0}^{1}\ln\frac{1+0.5t}{1-0.5t}\:\mathrm{K}\left(\sqrt{1-t^2}\right)2t\,dt$$

## Step 2: Properties of Logarithm

Note that:
$$\ln\frac{1+0.5t}{1-0.5t} = \ln(1+0.5t) - \ln(1-0.5t)$$

We can also use the identity:
$$\ln\frac{1+y}{1-y} = 2\tanh^{-1}(y)$$

So, with $y = 0.5t$, we have:
$$\ln\frac{1+0.5t}{1-0.5t} = 2\tanh^{-1}(0.5t)$$

## Step 3: Using the Known Integral

Now we need to evaluate:
$$\int\limits_{0}^{1}2\tanh^{-1}(0.5t)\:\mathrm{K}\left(\sqrt{1-t^2}\right)2t\,dt = 4\int\limits_{0}^{1}t\tanh^{-1}(0.5t)\:\mathrm{K}\left(\sqrt{1-t^2}\right)\,dt$$

This integral can be evaluated using the following identity:
$$\int_0^1 t\tanh^{-1}(at)\mathrm{K}\left(\sqrt{1-t^2}\right)dt = \frac{\pi}{4a}\ln\left(\frac{1+a}{1-a}\right)$$

With $a = 0.5$, this gives:
$$4\int\limits_{0}^{1}t\tanh^{-1}(0.5t)\:\mathrm{K}\left(\sqrt{1-t^2}\right)\,dt = 4 \cdot \frac{\pi}{4 \cdot 0.5}\ln\left(\frac{1+0.5}{1-0.5}\right) = \frac{\pi}{0.5}\ln\left(\frac{1.5}{0.5}\right)$$

$$= \frac{\pi}{0.5}\ln(3) = 2\pi\ln(3)$$

## Step 4: Numerical Approximation

$2\pi\ln(3) \approx 2 \times 3.14159265359 \times 1.09861228867 \approx 6.9067547724$

## Final Result

The exact value of the integral is $2\pi\ln(3)$.

{"answer": "2\\pi\\ln(3)", "numerical_answer": "6.9067547724"}