We wish to evaluate
  I = ∫₀^(2π) sin(sin x – x) dx.

Step 1. Rewrite the integrand using the sine difference formula:
  sin(sin x – x) = sin(sin x) cos x – cos(sin x) sin x.

Step 2. Instead of attacking the integral directly, consider a symmetry trick. Define
  I = ∫₀^(2π) sin(sin x – x) dx.
Now perform the substitution x' = 2π – x. Because dx = –dx', when x runs from 0 to 2π, x' runs from 2π to 0. Rewriting,
  I = ∫₂π⁰ sin(sin(2π – x') – (2π – x')) (–dx')
    = ∫₀^(2π) sin(sin(2π – x') – (2π – x')) dx'.
Note that sin(2π – x') = sin x' (using the periodicity and symmetry of sine) and also note that
  sin(sin(2π – x') – (2π – x')) = sin(sin x' – (2π – x'))
    = sin(sin x' + x' – 2π).
Because sine is 2π–periodic, sin(sin x' + x' – 2π) = sin(sin x' + x').
Thus after relabeling x' → x we have:
  I = ∫₀^(2π) sin(sin x + x) dx.

Step 3. Now, add the two representations of I:
  I + I = ∫₀^(2π)[sin(sin x – x) + sin(sin x + x)] dx.

The sum inside the integral can be simplified using the sine sum formula:
  sin(a – b) + sin(a + b) = 2 sin a cos b.
Here, a = sin x and b = x, so the sum becomes
  2 sin(sin x) cos x.
Thus,
  2I = ∫₀^(2π) 2 sin(sin x) cos x dx
    = 2 ∫₀^(2π) sin(sin x) cos x dx.
Dividing both sides by 2 gives:
  I = ∫₀^(2π) sin(sin x) cos x dx.

Step 4. Evaluate J = ∫₀^(2π) sin(sin x) cos x dx.
Notice that the derivative of cos(sin x) with respect to x is:
  d/dx cos(sin x) = – sin(sin x) cos x.
Thus,
  sin(sin x) cos x = – d/dx cos(sin x).
Hence,
  J = –∫₀^(2π) d/dx cos(sin x) dx = –[cos(sin x)]₀^(2π).

Now, sin(0) = 0 and sin(2π) = 0 so:
  [cos(sin x)]₀^(2π) = cos(sin(2π)) – cos(sin 0) = cos(0) – cos(0) = 1 – 1 = 0.
Thus, J = –0 = 0.

Step 5. Therefore, I = 0.

Step 6. The numerical approximation of 0 is clearly 0.0000000000 to 10 decimal places.

Final answer in JSON format:
{"answer": "$0$", "numerical_answer": "0.0000000000"}