Let's denote the integral as  
\[
I = \int_0^1 \frac{1}{x} \ln(1-x) \ln\left(\frac{1+\sqrt{1-x}}{\sqrt{x}}\right) dx
\]
First, rewrite the logarithm in the integrand:
\[
\ln\left(\frac{1+\sqrt{1-x}}{\sqrt{x}}\right)
= \ln(1+\sqrt{1-x}) - \frac{1}{2} \ln(x)
\]

Thus,
\[
I = \int_0^1 \frac{1}{x} \ln(1-x) \left[ \ln(1+\sqrt{1-x}) - \frac{1}{2}\ln x \right] dx
\]
\[
= \int_0^1 \frac{1}{x}\ln(1-x) \ln(1+\sqrt{1-x}) dx - \frac{1}{2} \int_0^1 \frac{1}{x}\ln(1-x) \ln x \; dx
\]
Let us call the first integral \( I_1 \) and the second one \( I_2 \):

\[
I_1 = \int_0^1 \frac{1}{x}\ln(1-x) \ln(1+\sqrt{1-x}) dx
\]
\[
I_2 = \int_0^1 \frac{1}{x}\ln(1-x) \ln x \; dx
\]

### Step 1: Compute \( I_2 \)

We can use the fact:
\[
\int_0^1 \frac{1}{x}\ln(1-x) \ln x \; dx = -\zeta(3)
\]
(Reference: Gradshteyn & Ryzhik 4.224.2)

### Step 2: Compute \( I_1 \)

Let us expand \( \ln(1-x) \):

\[
\ln(1-x) = -\sum_{n=1}^\infty \frac{x^n}{n}
\]

Thus,
\[
I_1 = \int_0^1 \frac{1}{x} \left( -\sum_{n=1}^\infty \frac{x^n}{n} \right) \ln(1+\sqrt{1-x}) dx
= -\sum_{n=1}^\infty \frac{1}{n} \int_0^1 x^{n-1} \ln(1+\sqrt{1-x}) dx
\]

Let:
\[
J_n = \int_0^1 x^{n-1} \ln(1+\sqrt{1-x}) dx
\]

We change variables: \( y = 1-x \implies x = 1-y, dx = -dy \), so as \( x: 0 \to 1 \), \( y: 1 \to 0 \):

\[
J_n = \int_1^0 (1-y)^{n-1} \ln(1+\sqrt{y}) (-dy) = \int_0^1 (1-y)^{n-1} \ln(1+\sqrt{y}) dy
\]

Thus:
\[
I_1 = -\sum_{n=1}^\infty \frac{1}{n} \int_0^1 (1-y)^{n-1} \ln(1+\sqrt{y}) dy
\]
\[
= -\int_0^1 \ln(1+\sqrt{y}) \left( \sum_{n=1}^\infty \frac{(1-y)^{n-1}}{n} \right) dy
\]

The sum can be written in terms of a logarithm:
\[
\sum_{n=1}^\infty \frac{t^{n-1}}{n} = \frac{-\ln(1-t)}{t}
\]
For \( t = 1-y \):
\[
\sum_{n=1}^\infty \frac{(1-y)^{n-1}}{n} = \frac{-\ln y}{1-y}
\]

So,
\[
I_1 = -\int_0^1 \ln(1+\sqrt{y}) \cdot \frac{-\ln y}{1-y} dy = \int_0^1 \frac{\ln(1+\sqrt{y}) \ln y}{1-y} dy
\]

Now, let’s set \( y = t^2 \), so \( t \in [0, 1] \), \( dy = 2t dt \), \( \sqrt{y} = t \):

\[
I_1 = \int_0^1 \frac{\ln(1+t) \ln(t^2)}{1-t^2} \cdot 2t dt
= 2 \int_0^1 \frac{\ln(1+t) \cdot 2\ln t \cdot t}{1-t^2} dt
\]
\[
= 4 \int_0^1 \frac{t \ln(1+t) \ln t}{1-t^2} dt
\]

But \(\ln (t^2) = 2\ln t\).

Now, \( \frac{t}{1-t^2} = \frac{1}{2} \left( \frac{1}{1-t} - \frac{1}{1+t} \right) \), so

\[
I_1 = 4 \int_0^1 \frac{t \ln(1+t) \ln t}{1-t^2} dt
= 2 \int_0^1 \frac{\ln(1+t)\ln t}{1-t} dt - 2 \int_0^1 \frac{\ln(1+t)\ln t}{1+t} dt
\]

Call these \( I_{1a} \) and \( I_{1b} \):

\[
I_{1a} = \int_0^1 \frac{\ln(1+t) \ln t}{1-t} dt
\]
\[
I_{1b} = \int_0^1 \frac{\ln(1+t) \ln t}{1+t} dt
\]

Thus,
\[
I_1 = 2 I_{1a} - 2 I_{1b}
\]

Let’s look for known values.

#### Compute \( I_{1b} \):

We know (see, e.g., Gradshteyn & Ryzhik or integral tables):
\[
\int_0^1 \frac{\ln(1+x)\ln x}{1+x} dx = -\frac{\pi^2}{12} \ln 2 + \frac{7}{8} \zeta(3)
\]

#### Compute \( I_{1a} \):

We can use the following (see e.g. [integral tables](https://en.wikipedia.org/wiki/List_of_integrals_of_logarithmic_functions)):
There are some relevant results:

There is a result:
\[
\int_0^1 \frac{\ln(1+x) \ln x}{1-x} dx = \frac{\pi^2}{12} \ln 2 - \frac{1}{4} \zeta(3)
\]

Thus,

\[
I_1 = 2 \left[ \frac{\pi^2}{12} \ln 2 - \frac{1}{4} \zeta(3) + \frac{\pi^2}{12} \ln 2 - \frac{7}{8} \zeta(3) \right]
= 2 \left( \frac{\pi^2}{6} \ln 2 - \frac{9}{8} \zeta(3) \right )
= \frac{\pi^2}{6} \ln 2 - \frac{9}{4} \zeta(3)
\]

But this seems inconsistent with the signs above for \(I_{1b}\). Let's recompute the expression:

Recall:
\[
I_{1a} = \frac{\pi^2}{12} \ln 2 - \frac{1}{4} \zeta(3)
\]
\[
I_{1b} = -\frac{\pi^2}{12} \ln 2 + \frac{7}{8} \zeta(3)
\]

So,
\[
I_1 = 2I_{1a} - 2I_{1b}
= 2 \left( \frac{\pi^2}{12}\ln 2 - \frac{1}{4}\zeta(3) \right )
- 2 \left( -\frac{\pi^2}{12}\ln 2 + \frac{7}{8}\zeta(3) \right )
\]
\[
= \frac{\pi^2}{6}\ln 2 - \frac{1}{2}\zeta(3) + \frac{\pi^2}{6}\ln 2 - \frac{7}{4}\zeta(3)
\]
\[
= \frac{\pi^2}{3}\ln 2 - 2\zeta(3)
\]

### Step 3: Assemble Full Result

Recall \(I_2 = -\zeta(3)\), so
\[
I = I_1 - \frac{1}{2}I_2 = \left( \frac{\pi^2}{3}\ln 2 - 2\zeta(3) \right ) - \frac{1}{2}(-\zeta(3))
= \frac{\pi^2}{3}\ln 2 - 2\zeta(3) + \frac{1}{2} \zeta(3)
= \frac{\pi^2}{3}\ln 2 - \frac{3}{2}\zeta(3)
\]

### Step 4: Numerical Evaluation

Let's plug in values:
- \( \pi^2 = 9.869604401089358 \)
- \( \ln 2 = 0.6931471805599453 \)
- \( \zeta(3) = 1.202056903159594 \)

Then,
\[
\frac{\pi^2}{3} \ln 2 = \frac{9.869604401089358}{3} \times 0.6931471805599453 = 3.289868133696453 \times 0.6931471805599453 \approx 2.2796955866
\]
\[
\frac{3}{2} \zeta(3) = 1.5 \times 1.202056903159594 = 1.8030853547
\]
\[
I \approx 2.2796955866 - 1.8030853547 = 0.4766102319
\]

### Final Answer (as JSON)

```json
{"answer": "\\frac{\\pi^2}{3}\\ln 2 - \\frac{3}{2}\\zeta(3)", "numerical_answer": "0.4766102319"}
```