Let's compute the definite integral:
\[
I = \int_{0}^{2} x^{-1/2}\, H_3\left(\sqrt[4]{x(2-x)}\right)\, dx,
\]
where \( H_3(x) \) is the 3rd Hermite polynomial.

---

### 1. Find \( H_3(x) \)

The Hermite polynomials (physicists' version) are:
\[
H_0(x) = 1 \\
H_1(x) = 2x \\
H_2(x) = 4x^2 - 2 \\
H_3(x) = 8x^3 - 12x
\]

---

### 2. Substitute \( H_3 \) into the integral

\[
I = \int_{0}^{2} x^{-1/2} \left[ 8\left(\sqrt[4]{x(2-x)}\right)^3 - 12\sqrt[4]{x(2-x)} \right] dx
\]

Now,
\[
\left(\sqrt[4]{x(2-x)}\right)^3 = \left(x(2-x)\right)^{3/4}
\]
\[
\sqrt[4]{x(2-x)} = \left(x(2-x)\right)^{1/4}
\]

So the integral becomes:
\[
I = 8\int_0^2 x^{-1/2}(x(2-x))^{3/4} dx - 12\int_0^2 x^{-1/2}(x(2-x))^{1/4} dx
\]

Let us write:
\[
I_1 = \int_0^2 x^{-1/2}(x(2-x))^{3/4} dx
\]
\[
I_2 = \int_0^2 x^{-1/2}(x(2-x))^{1/4} dx
\]

---

### 3. Use substitution \( x = 2y \), \( dx = 2dy \), \( x \in [0,2] \Rightarrow y \in [0,1] \)

Let \( x = 2y \Rightarrow x(2-x) = 2y(2-2y) = 4y(1-y) \).

So:
- \( x^{-1/2} = (2y)^{-1/2} = 2^{-1/2} y^{-1/2} \)
- \( (x(2-x))^{k} = (4y(1-y))^{k} = 4^k y^k (1-y)^k \)

Let's substitute in both integrals:

---

#### First integral (\( k = 3/4 \)):

\[
I_1 = \int_0^2 x^{-1/2}(x(2-x))^{3/4} dx = \int_0^1 (2^{-1/2} y^{-1/2}) (4^{3/4} y^{3/4} (1-y)^{3/4}) \cdot 2\, dy
\]

- \( 4^{3/4} = (2^2)^{3/4} = 2^{3/2} \)
- \( 2^{-1/2} \cdot 2 = 2^{1 - 1/2} = 2^{1/2} \)

So:
\[
I_1 = 2^{1/2} \cdot 2^{3/2} \int_0^1 y^{-1/2} y^{3/4} (1-y)^{3/4} dy
\]
\[
= 2^{2} \int_0^1 y^{-1/2+3/4} (1-y)^{3/4} dy
\]
\[
= 4 \int_0^1 y^{1/4} (1-y)^{3/4} dy
\]

---

#### Second integral (\( k = 1/4 \)):

\[
I_2 = \int_0^2 x^{-1/2}(x(2-x))^{1/4} dx = \int_0^1 (2^{-1/2} y^{-1/2}) (4^{1/4} y^{1/4} (1-y)^{1/4}) \cdot 2\, dy
\]

- \( 4^{1/4} = (2^2)^{1/4} = 2^{1/2} \)

So:
\[
I_2 = 2^{-1/2} \cdot 2^{1/2} \cdot 2 \int_0^1 y^{-1/2} y^{1/4} (1-y)^{1/4} dy = 2 \int_0^1 y^{-1/2 + 1/4} (1-y)^{1/4} dy
\]
\[
= 2 \int_0^1 y^{-1/4} (1-y)^{1/4} dy
\]

---

### 4. Substitute back into original integral

So,
\[
I = 8I_1 - 12 I_2 = 8 \times 4 \int_0^1 y^{1/4}(1-y)^{3/4}dy - 12\times 2 \int_0^1 y^{-1/4}(1-y)^{1/4}dy
\]
\[
= 32 \int_0^1 y^{1/4}(1-y)^{3/4}dy - 24 \int_0^1 y^{-1/4}(1-y)^{1/4}dy
\]

---

### 5. Express in terms of the Beta function

Recall:
\[
\int_0^1 y^{a-1} (1-y)^{b-1} dy = B(a,b) = \frac{\Gamma(a)\Gamma(b)}{\Gamma(a+b)}
\]
- \( \int_0^1 y^{1/4}(1-y)^{3/4}dy = B(\frac{5}{4}, \frac{7}{4}) \)
- \( \int_0^1 y^{-1/4}(1-y)^{1/4}dy = B(\frac{3}{4}, \frac{5}{4}) \)

Thus:
\[
I = 32 B(\frac{5}{4}, \frac{7}{4}) - 24 B(\frac{3}{4}, \frac{5}{4})
\]

Express Beta in terms of Gamma:
\[
B(a, b) = \frac{\Gamma(a)\Gamma(b)}{\Gamma(a+b)}
\]

So,
\[
I = 32 \frac{\Gamma(\frac{5}{4})\Gamma(\frac{7}{4})}{\Gamma(3)} - 24 \frac{\Gamma(\frac{3}{4})\Gamma(\frac{5}{4})}{\Gamma(2)}
\]

Recall \( \Gamma(2) = 1! = 1\) and \( \Gamma(3) = 2! = 2 \).

\[
I = 32 \frac{\Gamma(\frac{5}{4})\Gamma(\frac{7}{4})}{2} - 24 \Gamma(\frac{3}{4})\Gamma(\frac{5}{4})
\]
\[
= 16 \Gamma(\frac{5}{4})\Gamma(\frac{7}{4}) - 24 \Gamma(\frac{3}{4})\Gamma(\frac{5}{4})
\]
\[
= \Gamma\left(\frac{5}{4}\right) \left[ 16 \Gamma\left(\frac{7}{4}\right) - 24 \Gamma\left(\frac{3}{4}\right) \right]
\]

---

### 6. Numerical Approximation

Recall:
- \( \Gamma(\frac{5}{4}) \approx 0.9064024771 \)
- \( \Gamma(\frac{7}{4}) \approx 1.2254167025 \)
- \( \Gamma(\frac{3}{4}) \approx 1.2254167025 \) (since \( \Gamma(z) \) and \( \Gamma(1-z)\Gamma(z) = \pi/\sin(\pi z) \), but let's check directly)

But actually:
- \( \Gamma(0.75) \approx 1.225416703 \)
- \( \Gamma(1.25) \approx 0.9064024771 \)
- \( \Gamma(1.75) \approx 0.9181687424 \)

Thus:
- \( \Gamma(\frac{3}{4}) \approx 1.225416703 \)
- \( \Gamma(\frac{5}{4}) \approx 0.9064024771 \)
- \( \Gamma(\frac{7}{4}) \approx 1.225416703 \) (no, \( \Gamma(1.75) \approx 0.9181687424 \))

So list:
- \( \Gamma(0.75) \approx 1.225416703 \)
- \( \Gamma(1.25) \approx 0.9064024771 \)
- \( \Gamma(1.75) \approx 0.9181687424 \)

So:
\[
I_{num} = 16 \cdot 0.9064024771 \cdot 0.9181687424 - 24 \cdot 1.225416703 \cdot 0.9064024771
\]

First term:
- \( 0.9064024771 \times 0.9181687424 \approx 0.8320952749 \)
- \( 16 \times 0.8320952749 = 13.3135243984 \)

Second term:
- \( 1.225416703 \times 0.9064024771 \approx 1.110536140 \)
- \( 24 \times 1.110536140 = 26.65286736 \)

So,
\[
I_{num} = 13.3135243984 - 26.65286736 = -13.3393429616
\]

Rounded to 10 decimal places: \(-13.3393429616\)

---

### 7. Exact Answer

\[
\boxed{
I = 16 \Gamma\left(\frac{5}{4}\right)\Gamma\left(\frac{7}{4}\right) - 24 \Gamma\left(\frac{3}{4}\right)\Gamma\left(\frac{5}{4}\right)
}
\]

Or, factor \( \Gamma\left(\frac{5}{4}\right) \):
\[
I = \Gamma\left(\frac{5}{4}\right) \left[ 16 \Gamma\left(\frac{7}{4}\right) - 24 \Gamma\left(\frac{3}{4}\right) \right]
\]

---

### 8. Final output (in JSON):

```json
{"answer": "16 \\Gamma\\left(\\frac{5}{4}\\right)\\Gamma\\left(\\frac{7}{4}\\right) - 24 \\Gamma\\left(\\frac{3}{4}\\right)\\Gamma\\left(\\frac{5}{4}\\right)", "numerical_answer": "-13.3393429616"}
```