<think>
Okay, so I need to compute the definite integral from 0 to 1 of x squared times arccos x multiplied by the modified Bessel function of the first kind I0(2x). Hmm, that seems a bit complicated, but let's break it down step by step.

First, let me recall what I know about integrating functions involving arccos and Bessel functions. The arccos function can be tricky, but maybe I can use integration by parts. The Bessel function I0(2x) is a modified Bessel function of order 0. I remember that sometimes these functions can be expressed in terms of series expansions, which might be helpful here.

Let me write down the integral again: ∫₀¹ x² arccos(x) I₀(2x) dx. Let's think about integration by parts. Typically, integration by parts is useful when you have a product of functions where one part can be differentiated to simplify the integral. Here, arccos(x) is a good candidate for differentiation because its derivative is -1/√(1 - x²), which might simplify things. On the other hand, I₀(2x) is a Bessel function, and integrating it might not be straightforward. So maybe set u = arccos(x) and dv = x² I₀(2x) dx. Then du = -1/√(1 - x²) dx, and v would be the integral of x² I₀(2x) dx. But integrating x² I₀(2x) might not be simple. Let me check if I know any antiderivative for x² I₀(2x).

Alternatively, maybe expanding the Bessel function into its series representation would help. The modified Bessel function I₀(z) has a series expansion: I₀(z) = Σ [ (z/2)^(2k) / (k! Γ(k+1)) ) ] for k from 0 to ∞. Since here we have I₀(2x), substituting z = 2x gives I₀(2x) = Σ [ (x)^(2k) / (k! Γ(k+1)) ) ] * 2^(2k)/2^(2k) ? Wait, let me redo that. The general term is ( (z/2)^(2k) ) / (k! Γ(k+1)) ). So for z = 2x, that becomes ( (2x/2)^(2k) ) / (k! Γ(k+1)) ) = (x^(2k)) / (k! Γ(k+1)) ). But Γ(k+1) is just k! for integer k, so I₀(2x) = Σ [ x^(2k) / (k!)^2 ) ] summed from k=0 to ∞. That simplifies things a bit. So, I can write I₀(2x) as the sum from k=0 to infinity of x^(2k)/(k!)^2. Then, substituting this into the integral, the integral becomes the integral from 0 to 1 of x² arccos(x) times the sum over k of x^(2k)/(k!)^2 dx. Since the sum is uniformly convergent (I think Bessel functions have radius of convergence infinity, but here x is between 0 and 1, so it's definitely convergent), I can interchange the sum and the integral. So the integral becomes the sum over k from 0 to infinity of [1/(k!)^2] ∫₀¹ x^(2 + 2k) arccos(x) dx.

So now, the problem reduces to computing each integral ∫₀¹ x^(2 + 2k) arccos(x) dx for each k, then summing them multiplied by 1/(k!)^2. Let's focus on computing ∫ x^m arccos(x) dx, where m = 2 + 2k. Let's denote m as an even integer here. Let's consider substitution t = arccos(x). Then x = cos(t), and when x=0, t=π/2; when x=1, t=0. The integral becomes ∫_{π/2}^0 cos^m(t) * t * (-sin(t) dt) = ∫₀^{π/2} t cos^m(t) sin(t) dt. Hmm, that might be more manageable integral. Let's see. So, substituting t = arccos(x), dx = -sin(t) dt, and the limits invert. So the integral becomes ∫₀^{π/2} t cos^m(t) sin(t) dt. Let me check that substitution again. If x = cos(t), then dx = -sin(t) dt. So, when x=1, t=0; x=0, t=π/2. So the original integral from 0 to1 becomes integral from π/2 to 0, and the negative sign flips the limits back to 0 to π/2. So yes, the integral becomes ∫₀^{π/2} t cos^m(t) sin(t) dt.

Now, integrating t times cos^m(t) sin(t) dt. Let's consider integrating by parts here. Let u = t, dv = cos^m(t) sin(t) dt. Then du = dt, and v = -cos^{m+1}(t)/(m+1). Wait, integrating dv = cos^m(t) sin(t) dt. Let me check: Let’s set w = cos(t), then dw = -sin(t) dt. So, cos^m(t) sin(t) dt = -w^m dw. So integral of that is -w^{m+1}/(m+1) + C = -cos^{m+1}(t)/(m+1) + C. So yes, v = -cos^{m+1}(t)/(m+1). Therefore, integration by parts gives uv|₀^{π/2} - ∫₀^{π/2} v du. So:

∫ t cos^m(t) sin(t) dt = [ -t cos^{m+1}(t)/(m+1) ] from 0 to π/2 + ∫₀^{π/2} cos^{m+1}(t)/(m+1) dt.

Evaluating the boundary term: at π/2, cos(π/2) = 0, so the term is 0. At 0, cos(0) = 1, so the term is -0 * 1/(m+1) - [ -0 * ... ] Wait, actually, plugging in t=π/2: - (π/2) * 0^{m+1}/(m+1) = 0. At t=0: -0 * 1^{m+1}/(m+1) = 0. So the boundary term is 0. Therefore, the integral becomes [1/(m+1)] ∫₀^{π/2} cos^{m+1}(t) dt.

So, ∫₀¹ x^m arccos(x) dx = ∫₀^{π/2} t cos^m(t) sin(t) dt = [1/(m+1)] ∫₀^{π/2} cos^{m+1}(t) dt.

Therefore, the integral we need is [1/(m+1)] times the integral of cos^{m+1}(t) from 0 to π/2. Now, the integral of cos^n(t) from 0 to π/2 is known and is given by the beta function or the gamma function. Specifically, ∫₀^{π/2} cos^n(t) dt = (√π / 2) Γ((n+1)/2) / Γ((n+2)/2). Alternatively, using the formula for even and odd integers. Since m is 2 + 2k, which is even, m+1 is odd. Wait, m = 2 + 2k, so m+1 = 3 + 2k, which is odd. So n = m+1 = 3 + 2k. The integral ∫₀^{π/2} cos^{n}(t) dt for odd n can be expressed using the double factorial. For example, for n = 2k +1, the integral is ( (2k)!! / (2k +1)!! ) * π/2. Wait, but maybe I need to check the exact formula.

Wait, the standard result is that for integer n ≥ 0,

∫₀^{π/2} cos^{n}(t) dt = (π/2) * ( (n-1)!! / n!! ) ) if n is even,

and = ( (n-1)!! / n!! ) ) if n is odd.

Wait, let me confirm. For even exponents, the integral is (π/2) * ( (n-1)!! ) / n!! ), and for odd exponents, it's ( (n-1)!! ) / n!! ). So, for example, if n is even, say n=2m, then ∫₀^{π/2} cos^{2m}(t) dt = (π/2) * ( (2m -1)!! ) / (2m)!! )

If n is odd, say n=2m+1, then ∫₀^{π/2} cos^{2m+1}(t) dt = (2m)!! / (2m +1)!! )

So in our case, n = m +1 = 3 + 2k. Since m = 2 + 2k, so n = 3 + 2k, which is odd. Therefore, the integral ∫₀^{π/2} cos^{3 + 2k}(t) dt = ( (3 + 2k -1)!! ) / (3 + 2k)!! ) = ( (2k + 2)!! ) / (2k +3)!! )

Wait, let's check. For n odd, n=2m+1, then the integral is (2m)!! / (2m +1)!! ). So here, n=3 + 2k, which can be written as 2m +1 where m = (3 + 2k -1)/2 = (2 + 2k)/2 = 1 +k. Therefore, m =1 +k. Therefore, the integral is (2m)!! / (2m +1)!! ) = (2(1 +k))!! / (2(1 +k) +1)!! ) = (2k +2)!! / (2k +3)!! )

Therefore, ∫₀^{π/2} cos^{3 + 2k}(t) dt = (2k +2)!! / (2k +3)!! )

Therefore, going back, the integral ∫₀¹ x^{2 + 2k} arccos(x) dx = [1/(3 + 2k)] * (2k +2)!! / (2k +3)!! )

But wait, m =2 +2k, so m +1 =3 +2k. So the integral is [1/(3 +2k)] * (2k +2)!! / (2k +3)!! )

But now, we need to express this in terms of factorials or something else. Let's recall that for double factorials:

(2k +2)!! = 2^{k +1} (k +1)! )

Similarly, (2k +3)!! = (2k +3)(2k +1)...(3)(1) = product of odd numbers from 1 to 2k +3. Alternatively, (2k +3)!! = (2k +3)! ) / (2^{k +1} (k +1)! )

Wait, let me verify:

For even numbers: (2n)!! = 2^n n!

For odd numbers: (2n +1)!! = (2n +1)(2n -1)...3*1 = (2n +1)! ) / (2^n n! )

Yes, that's correct. So, (2k +2)!! = 2^{k +1} (k +1)! )

And (2k +3)!! = (2k +3)! ) / (2^{k +1} (k +1)! )

Therefore, (2k +2)!! / (2k +3)!! ) = [2^{k +1} (k +1)! ] / [ (2k +3)! / (2^{k +1} (k +1)! ) ) ] = [2^{k +1} (k +1)! ]^2 / (2k +3)! )

Therefore, the integral becomes [1/(3 +2k)] * [2^{2k +1)} (k +1)!^2 ] / (2k +3)! )

But let's see if we can simplify this expression. Let's write it as:

[1/(2k +3)] * [ (2k +2)!! / (2k +3)!! ) ]

But substituting the double factorial expressions:

= [1/(2k +3)] * [2^{k +1} (k +1)! ) / ( (2k +3)! ) / (2^{k +1} (k +1)! ) ) ]

Wait, this seems a bit messy. Maybe there's a better way to express this ratio. Let's take the original expression:

(2k +2)!! / (2k +3)!! ) = [2^{k +1} (k +1)! ] / [ (2k +3)! / (2^{k +1} (k +1)! ) ) ] = [2^{2k +2} (k +1)!^2 ] / (2k +3)! )

Therefore, the integral becomes [1/(2k +3)] * [2^{2k +2} (k +1)!^2 ] / (2k +3)! )

But (2k +3)! = (2k +3)(2k +2)! )

And (2k +2)! = (2k +2)(2k +1)! )

But perhaps this isn't helpful. Alternatively, let's note that (2k +3)! = (2k +3)(2k +2)(2k +1)! )

But maybe we can relate this to the gamma function. Alternatively, let's see if we can write this in terms of binomial coefficients or something else.

Alternatively, let's use the expression for the integral in terms of the Beta function. The integral ∫₀^{π/2} cos^{n}(t) dt can be expressed using the Beta function. Recall that:

∫₀^{π/2} cos^{n}(t) dt = (1/2) B( (n +1)/2, 1/2 )

Where B is the Beta function. And B(a,b) = Γ(a)Γ(b)/Γ(a +b). So, for n =3 +2k,

∫₀^{π/2} cos^{3 +2k}(t) dt = (1/2) B( (3 +2k +1)/2, 1/2 ) = (1/2) B( (4 +2k)/2, 1/2 ) = (1/2) B(2 +k, 1/2 )

Then, B(2 +k, 1/2 ) = Γ(2 +k)Γ(1/2)/Γ(2 +k +1/2 )

But Γ(1/2) = √π, and Γ(2 +k) = (k +1)! So,

B(2 +k, 1/2 ) = (k +1)! √π / Γ(2 +k +1/2 )

Therefore, the integral becomes (1/2) * (k +1)! √π / Γ(2 +k +1/2 )

But Γ(2 +k +1/2 ) = Γ( (k +2) +1/2 ) = (k +1 +1/2)(k +1/2)...(1/2) √π )

Wait, there's a formula for the Gamma function at half-integers. Γ(n +1/2) = (2n)! √π ) / 4^n n! )

But here, Γ(2 +k +1/2 ) = Γ( (k +2 ) +1/2 ) = ( (2(k +2) -1 )!! ) / 2^{k +2} ) √π )

Wait, let me check. For integer n ≥0,

Γ(n +1/2) = (2n)! / 4^n n! ) √π

So, for n =k +2,

Γ( (k +2 ) +1/2 ) = Γ( (k +2 ) +1/2 ) = (2(k +2) -1)!! / 2^{k +2} ) * √π )

Wait, but (2(k +2) -1)!! = (2k +3)!! )? Wait, no. Let's see, for n =k +2,

Γ(n +1/2) = Γ( (k +2 ) +1/2 ) = (2(k +2) -1)!! / 2^{k +2} ) * √π )

But (2(k +2) -1)!! = (2k +3)!! )

Yes, because 2(k +2) -1 =2k +4 -1=2k +3. So,

Γ(k +2 +1/2 ) = (2k +3)!! / 2^{k +2} ) * √π )

Therefore, substituting back into B(2 +k, 1/2 ):

B(2 +k, 1/2 ) = (k +1)! √π / [ (2k +3)!! / 2^{k +2} ) * √π ) ] = (k +1)! * 2^{k +2} / (2k +3)!! )

Therefore, the integral ∫₀^{π/2} cos^{3 +2k}(t) dt = (1/2) * (k +1)! * 2^{k +2} / (2k +3)!! ) = (k +1)! * 2^{k +1} / (2k +3)!! )

Therefore, going back to the original integral:

∫₀¹ x^{2 +2k} arccos(x) dx = [1/(2k +3)] * (k +1)! * 2^{k +1} / (2k +3)!! )

But (2k +3)!! = (2k +3)(2k +1)!! )

But (2k +1)!! = (2k +1)(2k -1)...3*1. Alternatively, using the relation (2k +3)!! = (2k +3)(2k +1)!! )

But perhaps this isn't helpful. Let's instead express (2k +3)!! in terms of factorials. As before, (2k +3)!! = (2k +3)! ) / (2^{k +1} (k +1)! )

Wait, let's check:

For n =k +1, (2n +1)!! = (2(k +1) +1)!! = (2k +3)!! = (2k +3)(2k +1)...3*1. Which is equal to (2k +3)! ) / (2^{k +1} (k +1)! )

Yes, because (2k +3)! = (2k +3)(2k +2)(2k +1)...2*1. If we separate the even and odd terms:

(2k +3)! = [ (2k +3)(2k +1)...3*1 ] * [ (2k +2)(2k)...2 ] = (2k +3)!! * 2^{k +1} (k +1)! )

Therefore, (2k +3)!! = (2k +3)! ) / (2^{k +1} (k +1)! )

Therefore, substituting back into the integral:

∫₀¹ x^{2 +2k} arccos(x) dx = [1/(2k +3)] * (k +1)! * 2^{k +1} / [ (2k +3)! / (2^{k +1} (k +1)! ) ) ]

= [1/(2k +3)] * (k +1)! * 2^{k +1} * 2^{k +1} (k +1)! / (2k +3)! )

= [1/(2k +3)] * [2^{2k +2} (k +1)!^2 ] / (2k +3)! )

But (2k +3)! = (2k +3)(2k +2)! )

And (2k +2)! = (2k +2)(2k +1)! )

But perhaps this is not helpful. Let's see if we can simplify the expression:

[2^{2k +2} (k +1)!^2 ] / [ (2k +3)! (2k +3) ) ]

But (2k +3)! = (2k +3)(2k +2)! )

So,

= [2^{2k +2} (k +1)!^2 ] / [ (2k +3)^2 (2k +2)! ) ]

But (2k +2)! = (2k +2)(2k +1)! )

= [2^{2k +2} (k +1)!^2 ] / [ (2k +3)^2 (2k +2)(2k +1)! ) ]

But (k +1)! = (k +1)k! )

Hmm, not sure. Alternatively, let's write (2k +2)! = (2k +2)(2k +1)(2k)! )

But this might not help. Alternatively, let's note that (2k +2)! = 2^{k +1} (k +1)! (2k +1)!! )

Wait, yes, because (2k +2)! = (2k +2)(2k +1)(2k)...2*1 = [2(k +1)][2k +1][2k]...[2*1] = 2^{k +1} (k +1)! ) * (2k +1)!! )

Therefore, (2k +2)! = 2^{k +1} (k +1)! (2k +1)!! )

Therefore, substituting back:

[2^{2k +2} (k +1)!^2 ] / [ (2k +3)^2 * 2^{k +1} (k +1)! (2k +1)!! ) ]

= [2^{2k +2} / 2^{k +1} ) ] * [ (k +1)!^2 / (k +1)! ) ] * [1 / ( (2k +3)^2 (2k +1)!! ) ) ]

= 2^{k +1} * (k +1)! / ( (2k +3)^2 (2k +1)!! ) )

Hmm, this seems complicated, but maybe there's a pattern here. Let's see if we can relate this to the original sum.

But perhaps this is getting too involved. Let's recall that the original integral is the sum over k of [1/(k!^2)] times this integral. So, putting it all together:

The integral ∫₀¹ x² arccos(x) I₀(2x) dx = Σ_{k=0}^∞ [1/(k!^2)] * [1/(2k +3)] * [ (2k +2)!! / (2k +3)!! ) ]

But substituting the expression we found earlier:

= Σ_{k=0}^∞ [1/(k!^2)] * [1/(2k +3)] * [ (2k +2)!! / (2k +3)!! ) ]

But perhaps there's a better way to express this sum. Let's try to write the terms in terms of factorials.

We have (2k +2)!! = 2^{k +1} (k +1)! )

And (2k +3)!! = (2k +3)(2k +1)!! = (2k +3)(2k +1)...(3)(1) )

But as before, (2k +3)!! = (2k +3)! ) / (2^{k +1} (k +1)! )

Therefore, (2k +2)!! / (2k +3)!! ) = [2^{k +1} (k +1)! ] / [ (2k +3)! / (2^{k +1} (k +1)! ) ) ] = [2^{2k +2} (k +1)!^2 ] / (2k +3)! )

Therefore, the term becomes:

[1/(k!^2)] * [1/(2k +3)] * [2^{2k +2} (k +1)!^2 ] / (2k +3)! )

= [2^{2k +2} (k +1)!^2 ] / [k!^2 (2k +3) (2k +3)! ) ]

= [2^{2k +2} (k +1)^2 ] / [ (2k +3) (2k +3)! ) ]

But (2k +3)! = (2k +3)(2k +2)(2k +1)! )

But (k +1)^2 / (2k +3)(2k +2)(2k +1)! ) Hmm, not sure.

Alternatively, let's write (k +1)! = (k +1)k! )

So, (k +1)!^2 = (k +1)^2 (k! )^2 )

Therefore, the term becomes:

[2^{2k +2} (k +1)^2 (k! )^2 ] / [k!^2 (2k +3) (2k +3)! ) ]

= [2^{2k +2} (k +1)^2 ] / [ (2k +3) (2k +3)! ) ]

But (2k +3)! = (2k +3)(2k +2)(2k +1)! )

So,

= [2^{2k +2} (k +1)^2 ] / [ (2k +3)^2 (2k +2)(2k +1)! ) ]

= [2^{2k +2} (k +1)^2 ] / [ (2k +3)^2k +2)(2k +1)! ) ]

But 2k +2 = 2(k +1), so:

= [2^{2k +2} (k +1)^2 ] / [ (2k +3) * 2(k +1) * (2k +1)! ) ]

= [2^{2k +2} (k +1) ] / [ 2(k +1) (2k +3) (2k +1)! ) ]

= [2^{2k +1} ] / [ (2k +3) (2k +1)! ) ]

Hmm, simplifying further:

= 2^{2k +1} / [ (2k +3) (2k +1)! ) ]

But 2^{2k +1} = 2 * 4^k * 2

Wait, 2^{2k +1} = 2 * (2^{2k}) = 2 * 4^k. Not sure. Alternatively, perhaps express (2k +1)! as (2k +1)(2k)! )

So,

= 2^{2k +1} / [ (2k +3) (2k +1)(2k)! ) ]

= 2^{2k +1} / [ (2k +1)(2k +3) (2k)! ) ]

But I'm not sure if this helps. Let's see if we can write this term in terms of binomial coefficients or something else.

Alternatively, perhaps we can recognize this sum as a hypergeometric function. The presence of factorials and powers suggests that this might be expressible in terms of a hypergeometric series.

Recall that the hypergeometric function _pF_q is defined as Σ [ (a_1)_n ... (a_p)_n / (b_1)_n ... (b_q)_n ) * z^n /n! ]

In our case, the term of the sum is:

Term_k = 2^{2k +1} / [ (2k +3) (2k +1)! ) ]

But let's write this as:

Term_k = 2^{2k +1} / [ (2k +3) (2k +1)! ) ] = 2^{2k +1} / [ (2k +3) (2k +1)! ) ]

Let me factor out constants. Let's note that 2^{2k +1} = 2 * 4^k. So:

Term_k = 2 * 4^k / [ (2k +3) (2k +1)! ) ]

But (2k +1)! = (2k +1)(2k)! )

So,

Term_k = 2 *4^k / [ (2k +3)(2k +1)(2k)! ) ]

But 4^k / (2k)! ) is similar to the terms in the expansion of cosh(2) or something, but with additional factors.

Alternatively, perhaps we can write this as:

Term_k = 2 / [ (2k +3)(2k +1) ) ] * (4^k)/(2k)! )

But 4^k/(2k)! ) is the term for cosh(2) or sinh(2), since cosh(z) = Σ_{k=0}^∞ z^{2k}/(2k)! ), so 4^k/(2k)! ) = (2^{2k})/(2k)! ) = (2^{2k})/(2k)! ), which is the term for cosh(2).

But here, we have an additional factor of 1/( (2k +3)(2k +1) )

So, the sum becomes:

Σ_{k=0}^∞ [2 / ( (2k +1)(2k +3) ) ] * (4^k)/(2k)! )

But this still doesn't ring a bell. Maybe integrating or differentiating known series.

Alternatively, consider that 1/( (2k +1)(2k +3) ) can be expressed as partial fractions:

1/( (2k +1)(2k +3) ) = (1/2)[ 1/(2k +1) - 1/(2k +3) ]

Yes, because:

(1/(2k +1) - 1/(2k +3)) = [ (2k +3) - (2k +1) ] / [ (2k +1)(2k +3) ] = 2 / [ (2k +1)(2k +3) ]

Therefore, 1/( (2k +1)(2k +3) ) = (1/2)(1/(2k +1) - 1/(2k +3) )

Therefore, the term becomes:

2 * (1/2)(1/(2k +1) - 1/(2k +3)) * (4^k)/(2k)! )

= [1/(2k +1) - 1/(2k +3) ] * (4^k)/(2k)! )

Therefore, the sum becomes:

Σ_{k=0}^∞ [1/(2k +1) - 1/(2k +3) ] * (4^k)/(2k)! )

This is a telescoping series? Let's check.

Let's split the sum into two parts:

Σ_{k=0}^∞ [4^k/( (2k +1)(2k)! ) ) ] - Σ_{k=0}^∞ [4^k/( (2k +3)(2k)! ) ) ]

Let's consider the first sum S1 = Σ_{k=0}^∞ 4^k/( (2k +1)(2k)! ) )

And the second sum S2 = Σ_{k=0}^∞ 4^k/( (2k +3)(2k)! ) )

Let's try to express S1 and S2 in terms of known functions.

For S1, note that 4^k = (2)^2k, so:

S1 = Σ_{k=0}^∞ (2)^{2k} / [ (2k +1)(2k)! ) ]

But (2k)! in the denominator. Let's write this as:

S1 = Σ_{k=0}^∞ (2^{2k} ) / ( (2k +1)(2k)! ) )

= Σ_{k=0}^∞ ( (2^{k})^2 ) / ( (2k +1)(2k)! ) )

But perhaps relate this to the series expansion of sinh or cosh. Recall that sinh(z) = Σ_{k=0}^∞ z^{2k +1}/( (2k +1)! ) )

Similarly, the integral of sinh(z) would give terms with (2k +1) in the denominator.

Alternatively, consider that:

∫₀² sinh(t) dt = Σ_{k=0}^∞ ∫₀² t^{2k +1}/( (2k +1)! ) dt = Σ_{k=0}^∞ 2^{2k +2}/( (2k +2)(2k +1)! ) )

But not sure. Alternatively, let's consider differentiating or integrating a known series.

Let me think. Let's consider the function f(z) = Σ_{k=0}^∞ z^{2k +1}/( (2k +1)(2k)! ) )

Then, f(z) = Σ_{k=0}^∞ z^{2k +1}/( (2k +1)(2k)! ) )

Let's compute the derivative f’(z):

f’(z) = Σ_{k=0}^∞ (2k +1) z^{2k}/( (2k +1)(2k)! ) ) = Σ_{k=0}^∞ z^{2k}/(2k)! ) = cosh(z)

Therefore, f(z) = ∫₀^z cosh(t) dt + C. Since f(0) =0, C=0. Therefore, f(z) = sinh(z).

Wait, but wait:

If f’(z) = cosh(z), then f(z) = sinh(z) + C. But f(0) =0, so C=0. Therefore, f(z) = sinh(z).

But according to the definition,

f(z) = Σ_{k=0}^∞ z^{2k +1}/( (2k +1)(2k)! ) ) = sinh(z)

But sinh(z) = Σ_{k=0}^∞ z^{2k +1}/( (2k +1)! ) )

Comparing the two series:

Σ_{k=0}^∞ z^{2k +1}/( (2k +1)(2k)! ) ) = sinh(z)

But sinh(z) = Σ_{k=0}^∞ z^{2k +1}/( (2k +1)! ) )

Therefore, this implies that:

Σ_{k=0}^∞ z^{2k +1}/( (2k +1)(2k)! ) ) = sinh(z)

But this is only possible if (2k +1)! = (2k +1)(2k)! ), which is true. Therefore, indeed, the series is sinh(z).

Therefore, f(z) = sinh(z). Therefore, substituting z=2,

Σ_{k=0}^∞ (2)^{2k +1}/( (2k +1)(2k)! ) ) = sinh(2)

But wait, our S1 is Σ_{k=0}^∞ 4^k/( (2k +1)(2k)! ) ) = Σ_{k=0}^∞ (2)^{2k}/( (2k +1)(2k)! ) )

Which is equal to (1/2) Σ_{k=0}^∞ (2)^{2k +1}/( (2k +1)(2k)! ) ) = (1/2) sinh(2)

Therefore, S1 = (1/2) sinh(2)

Similarly, let's compute S2 = Σ_{k=0}^∞ 4^k/( (2k +3)(2k)! ) )

Let’s make a substitution m =k +1. Then when k=0, m=1, and the sum becomes:

Σ_{m=1}^∞ 4^{m -1}/( (2(m) +1)(2(m -1))! ) )

= Σ_{m=1}^∞ 4^{m -1}/( (2m +1)(2m -2)! ) )

But this seems messy. Alternatively, let's factor out 4 from the exponent:

S2 = (1/4) Σ_{k=0}^∞ 4^{k +1}/( (2k +3)(2k)! ) )

= (1/4) Σ_{k=0}^∞ 4^{k +1}/( (2k +3)(2k)! ) )

Let’s consider the function g(z) = Σ_{k=0}^∞ z^{2k +3}/( (2k +3)(2k)! ) )

Then, g’(z) = Σ_{k=0}^∞ z^{2k +2}/( (2k)! ) )

= z^2 Σ_{k=0}^∞ z^{2k}/(2k)! ) = z^2 cosh(z)

Therefore, g(z) = ∫₀^z t^2 cosh(t) dt

But integrating t^2 cosh(t) dt would require integration by parts. Let's compute it:

Let’s compute ∫ t^2 cosh(t) dt. Let u = t^2, dv = cosh(t) dt. Then du = 2t dt, v = sinh(t).

So, ∫ t^2 cosh(t) dt = t^2 sinh(t) - 2 ∫ t sinh(t) dt

Now, compute ∫ t sinh(t) dt. Let u = t, dv = sinh(t) dt. Then du = dt, v = cosh(t).

So, ∫ t sinh(t) dt = t cosh(t) - ∫ cosh(t) dt = t cosh(t) - sinh(t) + C

Therefore, going back:

∫ t^2 cosh(t) dt = t^2 sinh(t) - 2 [ t cosh(t) - sinh(t) ] + C = t^2 sinh(t) - 2t cosh(t) + 2 sinh(t) + C

Therefore, g(z) = [t^2 sinh(t) - 2t cosh(t) + 2 sinh(t) ] from 0 to z

At t=0, the terms are 0, 0, and 0. So,

g(z) = z^2 sinh(z) - 2z cosh(z) + 2 sinh(z)

Therefore, g(z) = sinh(z)(z^2 + 2) - 2z cosh(z)

But g(z) = Σ_{k=0}^∞ z^{2k +3}/( (2k +3)(2k)! ) )

Therefore, substituting z=2,

Σ_{k=0}^∞ 2^{2k +3}/( (2k +3)(2k)! ) ) = sinh(2)(4 + 2) - 4 cosh(2) = 6 sinh(2) - 4 cosh(2)

But our S2 is (1/4) Σ_{k=0}^∞ 4^{k +1}/( (2k +3)(2k)! ) ) = (1/4) Σ_{k=0}^∞ (2^{2(k +1)} )/( (2k +3)(2k)! ) )

= (1/4) Σ_{k=0}^∞ 2^{2k +2}/( (2k +3)(2k)! ) )

= (1/4) * [ Σ_{k=0}^∞ (2^{2k +3} )/( (2k +3)(2k)! ) ) ] * (1/2)

Wait, no. Let's see:

4^{k +1} = 4*4^k = 4*(2^2)^k = 4*2^{2k} = 2^{2k +2}

Therefore, S2 = (1/4) Σ_{k=0}^∞ 2^{2k +2}/( (2k +3)(2k)! ) )

= (1/4) * [ Σ_{k=0}^∞ 2^{2k +3}/( (2k +3)(2k)! ) ) ] * (1/2)

Wait, no. Let's note that 2^{2k +2} = 2^{2k} * 4. So,

Σ_{k=0}^∞ 2^{2k +2}/( (2k +3)(2k)! ) ) = 4 Σ_{k=0}^∞ 2^{2k}/( (2k +3)(2k)! ) )

But this is 4 times the sum we computed earlier when we set z=2 in g(z). Wait, no. Wait, g(z) = Σ_{k=0}^∞ z^{2k +3}/( (2k +3)(2k)! ) )

So, if we set z=2, then g(2) = Σ_{k=0}^∞ 2^{2k +3}/( (2k +3)(2k)! ) ) = 6 sinh(2) -4 cosh(2)

Therefore, Σ_{k=0}^∞ 2^{2k +2}/( (2k +3)(2k)! ) ) = (1/2) Σ_{k=0}^∞ 2^{2k +3}/( (2k +3)(2k)! ) ) = (1/2) [6 sinh(2) -4 cosh(2) ]

Therefore, S2 = (1/4) * (1/2) [6 sinh(2) -4 cosh(2) ] = (1/8)(6 sinh(2) -4 cosh(2)) = (3/4) sinh(2) - (1/2) cosh(2)

Therefore, the original sum is S1 - S2 = (1/2 sinh(2)) - [ (3/4 sinh(2) -1/2 cosh(2) ) ] = (1/2 -3/4) sinh(2) +1/2 cosh(2) = (-1/4) sinh(2) +1/2 cosh(2)

Therefore, the integral ∫₀¹ x² arccos(x) I₀(2x) dx = (-1/4) sinh(2) + (1/2) cosh(2)

But cosh(2) - (1/2) sinh(2) ?

Wait, let's compute:

-1/4 sinh(2) +1/2 cosh(2) = (1/2 cosh(2) ) - (1/4 sinh(2) )

We can factor out 1/4:

= (1/4)(2 cosh(2) - sinh(2) )

Alternatively, express in terms of exponential functions:

cosh(2) = (e^2 + e^{-2})/2

sinh(2) = (e^2 - e^{-2})/2

Therefore,

2 cosh(2) - sinh(2) = 2*(e^2 + e^{-2})/2 - (e^2 - e^{-2})/2 = (e^2 + e^{-2}) - (e^2 - e^{-2})/2 = [2(e^2 + e^{-2}) - (e^2 - e^{-2}) ] / 2

= [2e^2 + 2e^{-2} -e^2 + e^{-2} ] /2 = [e^2 +3e^{-2} ] /2

Therefore,

(1/2 cosh(2) -1/4 sinh(2) ) = (1/4)(2 cosh(2) - sinh(2) ) = (1/4)( [e^2 +3e^{-2} ] /2 ) = (e^2 +3e^{-2}) /8

But let's compute this:

e^2 +3e^{-2} = e^2 +3/e^2 ≈ (7.38905609893) + 3/(7.38905609893) ≈7.38905609893 +0.4060058497 ≈7.7950619486

Then divided by 8: ≈0.974382743575

But let's check if this matches the numerical approximation.

Alternatively, perhaps there's a simpler expression. Let's see:

The integral result is (-1/4) sinh(2) + (1/2) cosh(2)

= (1/2 cosh(2) -1/4 sinh(2) )

= (2 cosh(2) - sinh(2) ) /4

But 2 cosh(2) - sinh(2) = cosh(2) + (cosh(2) - sinh(2) )

But cosh(2) - sinh(2) = e^{-2}

Therefore, 2 cosh(2) - sinh(2) = cosh(2) + e^{-2}

But cosh(2) = (e^2 + e^{-2})/2, so:

= (e^2 + e^{-2})/2 + e^{-2} = (e^2 + e^{-2} +2 e^{-2})/2 = (e^2 +3 e^{-2})/2

Therefore, the integral is (e^2 +3 e^{-2})/(8 )

So, the exact answer is (e² + 3e⁻²)/8.

Let me verify this:

We had the integral equal to (1/2 cosh(2) -1/4 sinh(2) )

Expressed in terms of exponentials:

cosh(2) = (e² + e⁻²)/2

sinh(2) = (e² - e⁻²)/2

Therefore,

1/2 cosh(2) = (e² + e⁻²)/4

1/4 sinh(2) = (e² - e⁻²)/8

Therefore,

1/2 cosh(2) -1/4 sinh(2) = (e² + e⁻²)/4 - (e² - e⁻²)/8 = [2(e² + e⁻²) - (e² - e⁻²) ] /8 = [2e² +2e⁻² -e² +e⁻² ] /8 = [e² +3e⁻² ] /8

Yes, so the exact value is (e² +3e⁻²)/8.

Therefore, the analytical result is (e² +3e⁻²)/8.

Now, let's compute the numerical approximation.

First, e² ≈7.38905609893

e⁻² ≈0.135335283237

Therefore,

e² +3e⁻² ≈7.38905609893 +3*0.135335283237 ≈7.38905609893 +0.406005849711 ≈7.79506194864

Divide by 8:7.79506194864 /8 ≈0.97438274358

Rounded to 10 decimal places:0.9743827436

But let me check with more precise values.

Using more precise e² and e⁻²:

e² ≈7.3890560989306495

e⁻² ≈0.1353352832366127

Then,

3e⁻² =0.4060058497098381

e² +3e⁻² =7.3890560989306495 +0.4060058497098381 ≈7.7950619486404876

Divide by8:7.7950619486404876 /8 ≈0.9743827435800609

Rounded to 10 decimal places:0.9743827436

Therefore, the numerical approximation is approximately 0.9743827436.

Therefore, the final answer is {"answer": "\frac{e^2 + 3e^{-2}}{8}", "numerical_answer": "0.9743827436"}

But let me check if there's a more simplified form. Alternatively, the exact answer can be written as (e² +3/e²)/8, which is the same as (e² +3e⁻²)/8.

Yes, that's correct.

So, the exact answer is (e² +3e⁻²)/8, and the numerical approximation is approximately 0.9743827436.
</think>

{"answer": "\\frac{e^2 + 3e^{-2}}{8}", "numerical_answer": "0.9743827436"}