<think>
Okay, let's tackle this integral step by step. The integral given is from 0 to 2 of x^(-1/2)(2 - x)^(-1/2)(1 + 0.5x)^(-2) T_{2×1}(√(1 + 0.5x)) dx. Hmm, first, I need to understand each part of this integrand.

Starting with the terms x^(-1/2) and (2 - x)^(-1/2). These look like parts of a Beta function integrand. The Beta function B(a, y) is ∫₀¹ t^(a-1)(1 - t)^(y-1) dt, which is related to the Gamma function. But here, the limits are from 0 to 2, so maybe a substitution can adjust the interval to [0,1]. Let me think about substitution. If I let t = x/2, then x = 2t, dx = 2dt. Then the limits become t=0 to t=1. Let's try that substitution first.

So substituting x = 2t, dx = 2dt. Then x^(-1/2) becomes (2t)^(-1/2) = (2)^(-1/2) t^(-1/2). Similarly, (2 - x)^(-1/2) becomes (2 - 2t)^(-1/2) = (2(1 - t))^(-1/2) = 2^(-1/2)(1 - t)^(-1/2). So multiplying these two terms: 2^(-1/2) * t^(-1/2) * 2^(-1/2) * (1 - t)^(-1/2) = 2^(-1) t^(-1/2)(1 - t)^(-1/2). Then the dx term is 2dt. So the product of all that would be 2^(-1) * 2 * t^(-1/2)(1 - t)^(-1/2) dt = t^(-1/2)(1 - t)^(-1/2) dt. That's the standard Beta function integrand, which is B(1/2, 1/2) when integrated from 0 to 1. But there's more to the integrand here.

The other part is (1 + 0.5x)^(-2) T_{2×1}(√(1 + 0.5x)). Let's parse this. First, (1 + 0.5x) is 1 + x/2. Then, T_{2×1}... Wait, T_{2×1} might be a typo or notation I'm not familiar with. Wait, the user wrote T_{2 × 1}(√(1 + 0.5x)). Maybe that's a function. Let me think. T could be the Chebyshev polynomial of the first kind, T_n(x). But here it's written as T_{2×1}, which is T_2? Because 2×1 is 2. Maybe it's a notation where T_{2×1} means T_2. Alternatively, maybe it's a tensor or something else, but in the context of integrals, Chebyshev polynomials are more plausible. Let me check the argument: √(1 + 0.5x). If T_2 is the Chebyshev polynomial of the first kind, then T_2(y) = 2y² - 1. Let's assume that T_{2×1} is a typo or notation for T_2. So substituting y = √(1 + 0.5x), then T_2(y) = 2y² - 1. Let's verify that.

If T_n(y) is the Chebyshev polynomial of the first kind, then T_2(y) = 2y² - 1. So if y = √(1 + 0.5x), then T_2(y) = 2(1 + 0.5x) - 1 = 2 + x - 1 = 1 + x. Wait, that simplifies nicely. So T_2(√(1 + 0.5x)) = 1 + x. Let me confirm that. Let's compute:

y = sqrt(1 + 0.5x) => y² = 1 + 0.5x. Then T_2(y) = 2y² - 1 = 2*(1 + 0.5x) - 1 = 2 + x -1 = 1 + x. Yes, that's correct. So the term T_{2×1}(sqrt(1 + 0.5x)) simplifies to 1 + x. Therefore, the integrand becomes:

x^(-1/2)(2 - x)^(-1/2) * (1 + 0.5x)^(-2) * (1 + x) dx.

So substituting back, the integral is from 0 to 2 of [x^(-1/2)(2 - x)^(-1/2) * [ (1 + x) / (1 + 0.5x)^2 ] dx.

Now, let's see if we can simplify this. Let's first note that 1 + 0.5x = 1 + x/2. So (1 + x/2)^2 is the denominator. Let's write the entire integrand:

x^{-1/2} (2 - x)^{-1/2} (1 + x) / (1 + x/2)^2 dx.

Hmm. Let's see if we can make a substitution here. Let me recall that after substitution x = 2t, the integral becomes from t=0 to t=1, and the integrand becomes t^{-1/2}(1 - t)^{-1/2} * (1 + 2t) / (1 + t)^2 * 2dt. Wait, no, let's redo the substitution properly.

Wait, earlier when we did x = 2t, then x = 2t, so 1 + x/2 = 1 + t. So (1 + x/2) becomes 1 + t. Similarly, 1 + x = 1 + 2t. So substituting into the integrand:

Original integrand after substitution x=2t:

x^{-1/2} (2 - x)^{-1/2} (1 + x) / (1 + x/2)^2 dx

= (2t)^{-1/2} (2 - 2t)^{-1/2} (1 + 2t) / (1 + t)^2 * 2 dt

Simplify each term:

(2t)^{-1/2} = 2^{-1/2} t^{-1/2}

(2 - 2t)^{-1/2} = (2(1 - t))^{-1/2} = 2^{-1/2} (1 - t)^{-1/2}

Multiply these two: 2^{-1} t^{-1/2} (1 - t)^{-1/2}

Then multiply by (1 + 2t)/(1 + t)^2 and 2 dt:

So total integrand becomes:

2^{-1} t^{-1/2}(1 - t)^{-1/2} * (1 + 2t)/(1 + t)^2 * 2 dt

The 2 and 2^{-1} cancel out, so we have:

t^{-1/2}(1 - t)^{-1/2} * (1 + 2t)/(1 + t)^2 dt

So the integral becomes ∫₀¹ t^{-1/2}(1 - t)^{-1/2} (1 + 2t)/(1 + t)^2 dt

Hmm. Now, this integral is from 0 to 1, and the t^{-1/2}(1 - t)^{-1/2} part is the Beta function integrand. But multiplied by (1 + 2t)/(1 + t)^2. Let's see if we can express (1 + 2t)/(1 + t)^2 in a more manageable form.

Let me compute (1 + 2t)/(1 + t)^2. Let's expand the denominator: (1 + t)^2 = 1 + 2t + t². The numerator is 1 + 2t. So (1 + 2t)/(1 + t)^2 = [1 + 2t]/[1 + 2t + t²]. Hmm, not sure if that helps. Alternatively, perhaps perform substitution u = t/(1 + t) or something else. Alternatively, maybe expand the fraction.

Alternatively, let's split the fraction:

(1 + 2t)/(1 + t)^2 = A/(1 + t) + B/(1 + t)^2. Let's try partial fractions.

Let’s set (1 + 2t)/(1 + t)^2 = A/(1 + t) + B/(1 + t)^2.

Multiply both sides by (1 + t)^2:

1 + 2t = A(1 + t) + B.

Expanding the right side: A + At + B.

So, equate coefficients:

For t term: 2 = A.

Constants: 1 = A + B. Since A=2, then B = 1 - 2 = -1.

Therefore, (1 + 2t)/(1 + t)^2 = 2/(1 + t) - 1/(1 + t)^2.

So the integral becomes:

∫₀¹ t^{-1/2}(1 - t)^{-1/2} [2/(1 + t) - 1/(1 + t)^2] dt

= 2 ∫₀¹ t^{-1/2}(1 - t)^{-1/2}/(1 + t) dt - ∫₀¹ t^{-1/2}(1 - t)^{-1/2}/(1 + t)^2 dt

So now we have two integrals to compute: let's call them I1 and I2.

I1 = ∫₀¹ t^{-1/2}(1 - t)^{-1/2}/(1 + t) dt

I2 = ∫₀¹ t^{-1/2}(1 - t)^{-1/2}/(1 + t)^2 dt

We need to compute 2I1 - I2.

Now, these integrals might be expressible in terms of Beta functions or hypergeometric functions, but I need to recall if there's a standard integral formula for such forms.

Alternatively, we can use substitution. Let me consider substitution for I1 and I2.

Let’s consider substitution u = t/(1 + t). Wait, or perhaps use substitution related to Beta function with parameters.

Alternatively, use substitution t = sin²θ. Let me try that. Let t = sin²θ, so dt = 2 sinθ cosθ dθ. When t=0, θ=0; t=1, θ=π/2.

Then, t^{-1/2} = (sin²θ)^{-1/2} = 1/sinθ

(1 - t)^{-1/2} = (cos²θ)^{-1/2} = 1/cosθ

So t^{-1/2}(1 - t)^{-1/2} dt = (1/sinθ)(1/cosθ)(2 sinθ cosθ dθ) = 2 dθ

So the integral I1 becomes:

∫0^{π/2} 2 dθ / (1 + sin²θ)

Similarly, I2 becomes ∫0^{π/2} 2 dθ / (1 + sin²θ)^2

Wait, that's a good simplification. Let's verify:

For I1:

Original substitution gives:

I1 = ∫₀¹ t^{-1/2}(1 - t)^{-1/2}/(1 + t) dt

After substitution t = sin²θ, dt = 2 sinθ cosθ dθ,

So:

I1 = ∫0^{π/2} [1/sinθ * 1/cosθ * 2 sinθ cosθ dθ] / (1 + sin²θ)

Simplify numerator:

[1/sinθ * 1/cosθ * 2 sinθ cosθ] = 2

So I1 = ∫0^{π/2} 2 / (1 + sin²θ) dθ

Similarly, I2:

I2 = ∫₀¹ t^{-1/2}(1 - t)^{-1/2}/(1 + t)^2 dt

After substitution:

I2 = ∫0^{π/2} 2 / (1 + sin²θ)^2 dθ

So now, we need to compute I1 and I2 as integrals over θ from 0 to π/2 of 2/(1 + sin²θ) and 2/(1 + sin²θ)^2.

Let’s compute I1 first.

I1 = 2 ∫0^{π/2} dθ / (1 + sin²θ)

To compute this integral, we can use the identity:

∫0^{π/2} dθ / (1 + a sin²θ) = π/(2√(1 + a))

But let's check. Let me recall that ∫0^{π/2} 1/(a + b sin²θ) dθ = π/(2√(a(a + b)))

Wait, let me verify. Let’s set a = 1, b = 1. Then ∫0^{π/2} 1/(1 + sin²θ) dθ.

Using substitution, let’s use t = tanθ, so θ from 0 to π/2 becomes t from 0 to ∞.

Then sinθ = t/√(1 + t²), dθ = dt/(1 + t²)

So integral becomes ∫0^∞ [1 / (1 + t²/(1 + t²))] * dt/(1 + t²)

Simplify denominator inside: 1 + t²/(1 + t²) = (1 + t² + t²)/(1 + t²) = (1 + 2t²)/(1 + t²)

So integral becomes (1 + t²)/(1 + 2t²) * dt/(1 + t²) = dt/(1 + 2t²)

Thus, ∫0^∞ dt/(1 + 2t²) = (1/√2) arctan(t√2) | from 0 to ∞ = (1/√2)(π/2 - 0) = π/(2√2)

Therefore, I1 = 2 * π/(2√2) = π/√2 ≈ 2.221441469

Wait, but let me check the formula again. If the integral ∫0^{π/2} dθ/(1 + sin²θ) = π/(2√2), then multiplying by 2 gives π/√2. So I1 = π/√2.

Similarly, for I2 = 2 ∫0^{π/2} dθ/(1 + sin²θ)^2. Let's compute this.

To compute ∫0^{π/2} dθ/(1 + sin²θ)^2, we can use a similar substitution. Let’s use t = tanθ again. Then sinθ = t/√(1 + t²), dθ = dt/(1 + t²). The integral becomes:

∫0^∞ [1 / (1 + t²/(1 + t²))^2] * dt/(1 + t²)

Simplify denominator inside: 1 + t²/(1 + t²) = (1 + 2t²)/(1 + t²)

So denominator squared is (1 + 2t²)^2/(1 + t²)^2

Thus, the integrand becomes (1 + t²)^2/(1 + 2t²)^2 * dt/(1 + t²) = (1 + t²)/(1 + 2t²)^2 dt

So the integral is ∫0^∞ (1 + t²)/(1 + 2t²)^2 dt

Let’s split the numerator: 1 + t² = (1 + 2t²) - t²

So integral becomes ∫0^∞ [ (1 + 2t²) - t² ] / (1 + 2t²)^2 dt = ∫0^∞ [1/(1 + 2t²) - t²/(1 + 2t²)^2 ] dt

Compute each part:

First integral: ∫0^∞ 1/(1 + 2t²) dt = (1/√2) * π/2

Second integral: ∫0^∞ t²/(1 + 2t²)^2 dt. Let’s use substitution u = t√2, so t = u/√2, dt = du/√2. Then integral becomes:

∫0^∞ (u²/2)/(1 + u²)^2 * du/√2 = (1/(2√2)) ∫0^∞ u²/(1 + u²)^2 du

The integral ∫0^∞ u²/(1 + u²)^2 du can be computed by substitution v = u, dv = du, but integrating by parts. Let’s set:

Let’s let v = u, dv = du

dw = u/(1 + u²)^2 du, then w = -1/(2(1 + u²))

Integration by parts: uv - ∫ w dv

But maybe another approach. Let’s note that ∫ u²/(1 + u²)^2 du = ∫ [1/(1 + u²) - 1/(1 + u²)^2 ] du

So split into two integrals:

∫0^∞ [1/(1 + u²) - 1/(1 + u²)^2 ] du

The first integral is π/2, the second integral is ∫0^∞ 1/(1 + u²)^2 du = π/4 (since ∫0^∞ dx/(1 + x²)^2 = π/4)

So the integral becomes π/2 - π/4 = π/4

Therefore, the second integral is (1/(2√2)) * π/4 = π/(8√2)

So putting it all together:

∫0^∞ [1/(1 + 2t²) - t²/(1 + 2t²)^2 ] dt = (π/(2√2)) - (π/(8√2))? Wait, no, wait:

Wait, the first integral was ∫0^∞ 1/(1 + 2t²) dt = (1/√2) * π/2 = π/(2√2)

The second integral was ∫0^∞ t²/(1 + 2t²)^2 dt = π/(8√2)

So the original integral is π/(2√2) - π/(8√2) = (4π - π)/(8√2) = 3π/(8√2)

Therefore, the integral ∫0^{π/2} dθ/(1 + sin²θ)^2 = 3π/(8√2)

Therefore, I2 = 2 * 3π/(8√2) = 3π/(4√2)

So now, going back to the original expression: 2I1 - I2 = 2*(π/√2) - 3π/(4√2) = (2π/√2) - (3π)/(4√2) = (8π/4√2 - 3π/4√2) = 5π/(4√2)

Simplify 5π/(4√2). Rationalizing the denominator: 5π/(4√2) = 5π√2/(4*2) = 5π√2/8

So the exact value of the integral is 5π√2/8.

Now, let's compute the numerical approximation. Let's calculate 5 * π * sqrt(2) / 8.

Wait, wait, 5π√2 divided by 8. Let's compute that:

π ≈ 3.1415926536

sqrt(2) ≈ 1.4142135624

So 5 * π * sqrt(2) ≈ 5 * 3.1415926536 * 1.4142135624 ≈ 5 * 4.442882908 ≈ 22.21441454

Then divide by 8: 22.21441454 / 8 ≈ 2.7768018175

Rounded to 10 decimal places: 2.7768018175 ≈ 2.7768018175

Wait, let me check the calculation again:

First, compute π * sqrt(2):

3.141592653589793 * 1.4142135623730951 ≈ 4.442882908158368

Multiply by 5: 4.442882908158368 * 5 ≈ 22.21441454079184

Divide by 8: 22.21441454079184 / 8 ≈ 2.77680181759898

So approximately 2.7768018176 when rounded to 10 decimal places.

Therefore, the exact answer is 5π√2/8, and the numerical approximation is approximately 2.7768018176.

Let me verify if there's any mistake in the steps. Let's recap:

1. Substituted x = 2t, transformed the integral into a Beta function form with additional terms.

2. Recognized T_{2×1} as Chebyshev polynomial T_2, which simplified to 1 + x.

3. Performed substitution x = 2t, leading to integral in terms of t from 0 to 1.

4. Split the integrand using partial fractions.

5. Transformed the integrals into trigonometric form using t = sin²θ.

6. Computed I1 and I2 using substitution tanθ = t, leading to integrals involving 1/(1 + 2t²) and 1/(1 + 2t²)^2.

7. Evaluated the integrals, leading to I1 = π/√2 and I2 = 3π/(4√2).

8. Calculated 2I1 - I2 = 5π√2/8.

9. Numerical evaluation gives approximately 2.7768018176.

All steps seem correct. Therefore, the final answer should be 5π√2/8 with the numerical value as calculated.
</think>

{"answer": "\\frac{5\\sqrt{2}\\pi}{8}", "numerical_answer": "2.7768018176"}