Let's define the integral:
\[
I = \int_0^1 \sqrt[3]{x} \left\lfloor \frac{1}{\sqrt[3]{x}} \right\rfloor \, dx
\]

Let \( y = \sqrt[3]{x} \), so \( x = y^3 \), \( dx = 3y^2 dy \).

When \( x = 0 \), \( y = 0 \).  
When \( x = 1 \), \( y = 1 \).

So,
\[
I = \int_{y=0}^1 y \left\lfloor \frac{1}{y} \right\rfloor 3y^2 \, dy = 3\int_0^1 y^3 \left\lfloor \frac{1}{y} \right\rfloor \, dy
\]

Now \( \left\lfloor \frac{1}{y} \right\rfloor \) is constant (an integer \( n \)) for \( y \in \left( \frac{1}{n+1}, \frac{1}{n} \right] \) for \( n = 1,2,3,\ldots \).

Let’s break the integral into these steps:
\[
I = 3\sum_{n=1}^{\infty} \int_{y=1/(n+1)}^{y=1/n} y^3 n\, dy
\]
\[
= 3\sum_{n=1}^{\infty} n \int_{1/(n+1)}^{1/n} y^3 \, dy
\]

The indefinite integral:
\[
\int y^3 \, dy = \frac{y^4}{4}
\]

So:
\[
I = 3\sum_{n=1}^{\infty} n \left[ \frac{y^4}{4} \Bigg|_{y=1/(n+1)}^{y=1/n} \right]
\]
\[
= 3\sum_{n=1}^{\infty} n \left( \frac{1}{4} \left( \frac{1}{n^4} - \frac{1}{(n+1)^4} \right) \right)
\]
\[
= \frac{3}{4}\sum_{n=1}^{\infty} n \left( \frac{1}{n^4} - \frac{1}{(n+1)^4} \right)
\]

Let's expand \( n \left(\frac{1}{n^4} - \frac{1}{(n+1)^4} \right) \):
\[
n \left( \frac{1}{n^4} - \frac{1}{(n+1)^4} \right) = \frac{1}{n^3} - \frac{n}{(n+1)^4}
\]

So,
\[
I = \frac{3}{4} \left( \sum_{n=1}^{\infty} \frac{1}{n^3} - \sum_{n=1}^{\infty} \frac{n}{(n+1)^4} \right)
\]

The first sum is \(\zeta(3)\), Apery's constant.  
Evaluate the second sum:

Let’s write \( \frac{n}{(n+1)^4} = \frac{n+1-1}{(n+1)^4} = \frac{1}{(n+1)^3} - \frac{1}{(n+1)^4} \):

\[
\sum_{n=1}^\infty \frac{n}{(n+1)^4} = \sum_{n=1}^\infty \left( \frac{1}{(n+1)^3} - \frac{1}{(n+1)^4} \right)
= \sum_{k=2}^\infty \frac{1}{k^3} - \sum_{k=2}^\infty \frac{1}{k^4}
\]
(where \(k=n+1\))

So,
\[
\sum_{n=1}^\infty \frac{n}{(n+1)^4} = \left( \sum_{k=1}^\infty \frac{1}{k^3} - 1 \right) - \left( \sum_{k=1}^\infty \frac{1}{k^4} - 1 \right)
= (\zeta(3) - 1) - (\zeta(4) - 1) = \zeta(3) - \zeta(4)
\]

Thus,
\[
I = \frac{3}{4}\left( \zeta(3) - [\zeta(3) - \zeta(4)] \right) = \frac{3}{4} \zeta(4)
\]

But \(\zeta(4) = \frac{\pi^4}{90}\)

So the exact result:
\[
I = \frac{3}{4} \cdot \frac{\pi^4}{90} = \frac{\pi^4}{120}
\]

Numerical answer:
\[
\pi^4 \approx 97.4090910349
\]
\[
I = \frac{97.4090910349}{120} \approx 0.8117424253
\]

Thus:

```json
{"answer": "\\frac{\\pi^4}{120}", "numerical_answer": "0.8117424253"}
```