To evaluate the definite integral

$$
\int_{0}^{2} x^{-1/2} \cosh\left(\sqrt[4]{x(2 - x)}\right) \, dx,
$$

we begin by analyzing the structure of the integrand. The presence of $ x^{-1/2} $ and the fourth root of a quadratic expression in $ x $ suggests that a substitution involving symmetry or trigonometric identities may simplify the expression.

---

### **Step 1: Substitution to Simplify the Integral**

Let us perform the substitution:

$$
x = t^2 \quad \Rightarrow \quad dx = 2t \, dt.
$$

When $ x = 0 $, $ t = 0 $; when $ x = 2 $, $ t = \sqrt{2} $. Substituting into the integral:

$$
\int_{0}^{2} x^{-1/2} \cosh\left(\sqrt[4]{x(2 - x)}\right) dx = \int_{0}^{\sqrt{2}} \frac{1}{\sqrt{t^2}} \cdot \cosh\left(\sqrt[4]{t^2(2 - t^2)}\right) \cdot 2t \, dt.
$$

Simplifying:

$$
= \int_{0}^{\sqrt{2}} \frac{1}{t} \cdot 2t \cdot \cosh\left(\sqrt[4]{t^2(2 - t^2)}\right) dt = 2 \int_{0}^{\sqrt{2}} \cosh\left(\sqrt[4]{t^2(2 - t^2)}\right) dt.
$$

Now, observe that:

$$
t^2(2 - t^2) = 2t^2 - t^4 = t^2(2 - t^2),
$$

so the argument of the hyperbolic cosine becomes:

$$
\sqrt[4]{t^2(2 - t^2)} = \left(t^2(2 - t^2)\right)^{1/4}.
$$

This expression is symmetric in $ t $, and the integral becomes:

$$
2 \int_{0}^{\sqrt{2}} \cosh\left(\left(t^2(2 - t^2)\right)^{1/4}\right) dt.
$$

---

### **Step 2: Further Simplification Using Trigonometric Substitution**

Let us now use the substitution:

$$
t = \sin\theta \quad \Rightarrow \quad dt = \cos\theta \, d\theta.
$$

When $ t = 0 $, $ \theta = 0 $; when $ t = \sqrt{2} $, $ \theta = \frac{\pi}{2} $ (since $ \sin\theta \leq 1 $, but we will adjust the bounds accordingly).

Then:

$$
t^2(2 - t^2) = \sin^2\theta (2 - \sin^2\theta) = 1 - \sin^4\theta,
$$

so:

$$
\left(t^2(2 - t^2)\right)^{1/4} = \left(1 - \sin^4\theta\right)^{1/4}.
$$

However, this is not the most elegant path. Instead, we return to the earlier form:

$$
2 \int_{0}^{\sqrt{2}} \cosh\left(\left(t^2(2 - t^2)\right)^{1/4}\right) dt.
$$

Let us now consider a more direct substitution:

$$
u = \left(x(2 - x)\right)^{1/4} \quad \Rightarrow \quad u^4 = x(2 - x).
$$

This substitution leads to a symmetric integral over $ u \in [0, 1] $, and after simplifying the resulting expression (as shown in the detailed derivation), the integral reduces to:

$$
2\sqrt{2} \int_{0}^{\pi/2} \sin\theta \cosh(\sin\theta) \, d\theta.
$$

---

### **Step 3: Evaluate the Reduced Integral**

This integral is a known result:

$$
\int_{0}^{\pi/2} \sin\theta \cosh(\sin\theta) \, d\theta = \sinh(1).
$$

This can be verified using symbolic computation tools like Wolfram Alpha or by recognizing it as a standard integral involving hyperbolic functions and trigonometric