Let’s denote the integral by \( I \):
\[
I = \int_0^1 x \sin(x) \ln\left( \frac{1+\sqrt{1-x^2}}{1-\sqrt{1-x^2}} \right) dx
\]

**Step 1: Simplify the logarithmic term**

Note that:
\[
\ln\left( \frac{1+\sqrt{1-x^2}}{1-\sqrt{1-x^2}} \right) = 2 \, \text{arctanh} \left( \sqrt{1-x^2} \right)
\]
But also,
\[
\text{arctanh}(z) = \frac{1}{2} \ln \left( \frac{1+z}{1-z} \right)
\]
So,
\[
\ln\left( \frac{1+\sqrt{1-x^2}}{1-\sqrt{1-x^2}} \right) = 2\arctanh(\sqrt{1-x^2})
\]

But there is a classic identity:
\[
\arctanh(\sqrt{1-x^2}) = \text{arccosh}\left(\frac{1}{x}\right)
\]
for \( 0 < x \leq 1 \), where \(\text{arccosh}(y)\) is the inverse hyperbolic cosine.

Indeed,
\[
\text{arccosh}(z) = \ln(z + \sqrt{z^2 - 1})
\]
Set \(z = 1/x\):
\[
\sqrt{z^2 - 1} = \sqrt{(1/x^2) - 1} = \sqrt{\frac{1 - x^2}{x^2}} = \frac{\sqrt{1 - x^2}}{x}
\]
Thus,
\[
\ln \left( \frac{1}{x} + \frac{\sqrt{1-x^2}}{x} \right) = \ln \left( \frac{1 + \sqrt{1-x^2}}{x} \right)
\]

But let's return to the original form. Another useful substitution is \( x = \sin\theta \), for \( 0 \leq \theta \leq \frac{\pi}{2} \):

- \( x = \sin\theta \)
- \( dx = \cos\theta \, d\theta \)
- \( \sqrt{1 - x^2} = \cos\theta \)

Now,
\[
\ln\left( \frac{1+\cos\theta}{1-\cos\theta} \right) = \ln\left( \frac{2\cos^2(\theta/2)}{2\sin^2(\theta/2)} \right) = \ln\left(\cot^2(\theta/2)\right) = 2\ln\cot(\theta/2)
\]
But since \(\cot(\theta/2) = \frac{\cos(\theta/2)}{\sin(\theta/2)}\)

Now let’s write everything in terms of \(\theta\):

- \( x = \sin\theta \)
- \( dx = \cos\theta\, d\theta \)
- \( x\sin x = \sin\theta \cdot \sin(\sin\theta) \) — but this is more complicated than the original.
- But our original integral (with variable 1.0 written as just 1) is:
\[
I = \int_0^1 x \sin(x) \ln\left( \frac{1+\sqrt{1-x^2}}{1-\sqrt{1-x^2}} \right) dx
\]

But, as above,
\[
\ln\left( \frac{1+\sqrt{1-x^2}}{1-\sqrt{1-x^2}} \right) = 2 \arctanh(\sqrt{1-x^2})
\]

Thus,
\[
I = 2\int_0^1 x \sin x \arctanh(\sqrt{1-x^2}) dx
\]

Alternatively, for the domain \( x = \sin\theta, 0 \leq \theta \leq \pi/2 \), \( dx = \cos\theta d\theta \):

Let’s change the variable:

- \( x = \sin\theta \)
- \( dx = \cos\theta d\theta \)
- When \( x = 0, \theta = 0 \); when \( x = 1, \theta = \pi/2 \)
- \(\sqrt{1 - x^2} = \cos\theta \)

Moreover,
\[
I = \int_0^1 x \sin x \ln \left( \frac{1+\sqrt{1-x^2}}{1-\sqrt{1-x^2}} \right) dx
\]
We can write this as:
\[
I = \int_{\theta=0}^{\pi/2} \sin\theta \sin(\sin\theta) \ln\left( \frac{1+\cos\theta}{1-\cos\theta} \right) \cos\theta d\theta
\]
But \(\sin\theta \cos\theta = \frac{1}{2} \sin 2\theta\), so:
\[
I = \int_0^{\pi/2} \sin(\sin\theta) \sin\theta \cos\theta \ln\left( \frac{1+\cos\theta}{1-\cos\theta} \right) d\theta
= \frac{1}{2} \int_0^{\pi/2} \sin(\sin\theta) \sin 2\theta \ln\left( \frac{1+\cos\theta}{1-\cos\theta} \right) d\theta
\]

But now this is still a complex form due to \(\sin(\sin\theta)\).

Alternatively, let’s see if we can integrate \( x \sin x \ln \left( \frac{1+\sqrt{1-x^2}}{1-\sqrt{1-x^2}}\right) \) directly by parts.

Let’s set:
- \( u = \ln\left( \frac{1+\sqrt{1-x^2}}{1-\sqrt{1-x^2}} \right) \)
- \( dv = x \sin x dx \)

Compute \( dv \):
\[
\int x \sin x dx
\]
Let’s integrate by parts:
Let \( a = x \), \( db = \sin x dx \) \( \rightarrow da = dx \), \( b = -\cos x \)

\[
\int x \sin x dx = -x \cos x + \int \cos x dx = -x \cos x + \sin x + C
\]
Therefore,
\[
\int x \sin x dx = -x \cos x + \sin x
\]

Let’s use integration by parts for the original integral, with:
- \( u = \ln\left( \frac{1+\sqrt{1-x^2}}{1-\sqrt{1-x^2}} \right) \), so \( du = \frac{d}{dx}\left(\ln \left( \frac{1+\sqrt{1-x^2}}{1-\sqrt{1-x^2}}\right) \right) dx \)
- \( dv = x \sin x dx \), \( v = -x \cos x + \sin x \)

Then,
\[
I = \left[ u v \right]_0^1 - \int_0^1 v du
\]

Let’s compute the terms:

At \( x = 1 \):
- \(\sqrt{1-1^2} = 0\)
- \(\ln\left( \frac{1+0}{1-0} \right) = \ln(1) = 0\)
Thus, \(u(1) = 0\)

At \( x = 0 \):
- \(\sqrt{1-0^2} = 1\)
- \(\ln\left( \frac{1+1}{1-1} \right) = \ln\left( \frac{2}{0} \right) \rightarrow \infty \). But, \(x\) in the \(v\) term is zero, and \(\sin 0 = 0\).
- So, \(v(0) = -0 \cdot \cos 0 + \sin 0 = 0\)

Thus,
\[
\left[ u v \right]_0^1 = 0 - 0 = 0
\]

Therefore,
\[
I = - \int_0^1 v du
\]
where \( v = -x \cos x + \sin x \)

Let’s compute \( du \):

Recall,
\[
u = \ln\left( \frac{1+\sqrt{1-x^2}}{1-\sqrt{1-x^2}} \right)
\]
Let’s denote \( s = \sqrt{1-x^2} \), then:
\[
u(x) = \ln \left( \frac{1+s}{1-s} \right)
\]
Then:
\[
\frac{d}{dx} u(x) = \frac{1}{1+s} \cdot \frac{ds}{dx} - \frac{1}{1-s}\cdot \frac{ds}{dx}
= \left( \frac{1}{1+s} - \frac{1}{1-s} \right) \frac{ds}{dx}
\]

But,
\[
\frac{1}{1+s} - \frac{1}{1-s} = \frac{(1-s) - (1+s)}{(1+s)(1-s)} = \frac{1-s-1-s}{1-s^2} = \frac{-2s}{1 - s^2}
\]

But,
\[
0 \leq x \leq 1 \implies 1 - x^2 \geq 0,\, x \in [0, 1]
\]
Moreover, \( s = \sqrt{1 - x^2} \), so \( 1 - s^2 = 1 - (1 - x^2) = x^2 \)

Also,
\[
\frac{ds}{dx} = \frac{1}{2}(1-x^2)^{-1/2} \cdot (-2x) = -\frac{x}{\sqrt{1-x^2}}
\]

So,

\[
\frac{d}{dx}u(x) = \frac{-2s}{x^2} \cdot \left( -\frac{x}{\sqrt{1-x^2}} \right ) = \frac{2s}{x^2} \cdot \frac{x}{\sqrt{1-x^2}} = \frac{2sx}{x^2 \sqrt{1-x^2}}
\]

But \( s = \sqrt{1-x^2} \), so:

\[
\frac{d}{dx} u(x) = \frac{2\sqrt{1-x^2} \cdot x}{x^2 \sqrt{1-x^2}} = \frac{2x}{x^2} = \frac{2}{x}
\]
But that can't be possible for all \( x \)!

Wait. Let's carefully proceed.

Recall:
\[
u(x) = \ln \left( \frac{1+s}{1-s} \right ),\quad s = \sqrt{1-x^2}
\]
Then,
\[
\frac{d}{dx} u(x) = \frac{1}{\frac{1+s}{1-s}} \cdot \frac{d}{dx} \left( \frac{1+s}{1-s} \right )
= \frac{1-s}{1+s} \cdot \frac{d}{dx} \left( \frac{1+s}{1-s} \right )
\]

But a simpler way is as previously outlined:

Let’s set \(s = \sqrt{1-x^2}\), and note that \(1-s^2 = x^2\), so:

- \( \frac{ds}{dx} = -x / s \)
- \( \frac{1}{1+s} - \frac{1}{1-s} = -2s / x^2 \)

Therefore:

\[
\frac{d}{dx} u(x) = \left(\frac{1}{1+s} - \frac{1}{1-s}\right) \frac{ds}{dx} = \left( -\frac{2s}{x^2} \right) \left(-\frac{x}{s} \right) = \frac{2x}{x^2} = \frac{2}{x}
\]
This is a striking simplification!

Thus,
\[
\frac{d}{dx} \ln\left( \frac{1+\sqrt{1-x^2}}{1-\sqrt{1-x^2}} \right) = \frac{2}{x}
\]

Therefore,
\[
du = \frac{2}{x} dx
\]

Now, \( v = -x\cos x + \sin x \):

\[
I = - \int_0^1 (-x \cos x + \sin x) \frac{2}{x} dx = 2 \int_0^1 \left( \cos x - \frac{\sin x}{x} \right) dx
\]

**Therefore:**
\[
I = 2 \int_0^1 \cos x dx - 2 \int_0^1 \frac{\sin x}{x} dx
\]

Let’s evaluate these integrals:

- \( \int_0^1 \cos x dx = \sin x \Big|_0^1 = \sin 1 - 0 = \sin 1 \)
- \( \int_0^1 \frac{\sin x}{x} dx = \text{Si}(1) \), where \(\text{Si}(x)\) is the sine integral function.

So, the exact symbolic answer is:
\[
\boxed{
I = 2 \left( \sin 1 - \text{Si}(1) \right)
}
\]

**Step 3: Numerical approximation**

Let’s compute:

- \( \sin 1 \approx 0.8414709848 \)
- \( \text{Si}(1) \approx 0.9460830704 \)

So:
\[
I \approx 2 \times (0.8414709848 - 0.9460830704) = 2 \times (-0.1046120856) = -0.2092241712
\]

Rounded to 10 decimal places: \(\boxed{-0.2092241712}\)

**Step 4: Final JSON answer**

```json
{"answer": "2\\left(\\sin 1-\\operatorname{Si}(1)\\right)", "numerical_answer": "-0.2092241712"}
```