Let's solve the integral:
\[
I = \int_{0}^{2} x \arctan(\sqrt{x(2-x)})\,dx
\]

**Step 1: Substitution**

Let \( x = 2\sin^2\theta \), for \( \theta \in [0, \frac{\pi}{2}] \).

Then,

\[
dx = 4\sin\theta\cos\theta\,d\theta = 2\sin(2\theta)d\theta
\]

Also,

\[
x(2-x) = 2\sin^2\theta(2-2\sin^2\theta) = 4\sin^2\theta\cos^2\theta = (\sin(2\theta))^2
\]
So,
\[
\sqrt{x(2-x)} = |\sin(2\theta)| = \sin(2\theta)
\]
(because \(\theta \in [0, \pi/2]\), \(2\theta \in [0, \pi]\), so \(\sin(2\theta)\) is non-negative.)

Thus,

\[
I = \int_{x=0}^{x=2} x \arctan(\sqrt{x(2-x)})\,dx
\]
When \( x=0 \), \( \theta=0 \), \(x=2\), \(\theta=\frac{\pi}{2}\).

So,
\[
I = \int_{\theta=0}^{\pi/2} (2\sin^2\theta)\cdot \arctan(\sin(2\theta)) \cdot 2\sin(2\theta)d\theta
\]
\[
= 4\int_{0}^{\pi/2} \sin^2\theta \arctan(\sin(2\theta)) \sin(2\theta) d\theta
\]

But \(\sin^2\theta \sin(2\theta) = \sin^2\theta \cdot 2\sin\theta\cos\theta = 2\sin^3\theta\cos\theta\).

So
\[
I = 4 \int_{0}^{\pi/2} 2\sin^3\theta\cos\theta \arctan(\sin(2\theta)) d\theta = 8\int_{0}^{\pi/2} \sin^3\theta\cos\theta \arctan(\sin(2\theta)) d\theta
\]

**Step 2: Further substitution**

Let \( u = \sin(2\theta) \). Thus,

- When \( \theta = 0 \), \( u=0 \);
- When \( \theta = \frac{\pi}{2} \), \( u = \sin(\pi) = 0 \);
- However, as \( \theta \) goes from \( 0 \to \pi/2 \), \( \sin(2\theta) \) goes from 0 up to 1 at \( \theta=\pi/4 \) and back to 0 at \( \theta=\pi/2 \).

Alternatively, instead of substituting, let's try integrating by parts.

**Step 3: Integration by parts**

Let:

- \( u = \arctan(\sqrt{x(2-x)}) \)
- \( dv = x dx \)

Then,

- \( du = \frac{1}{1 + x(2-x)} \cdot \frac{d}{dx}(\sqrt{x(2-x)}) dx \)

But the derivative may be cumbersome.

Instead, observe this symmetric region \( x \to 2-x \), as:

\( \sqrt{x(2-x)} = \sqrt{(2-x)x} = \sqrt{x(2-x)} \)

Let us try substituting \( x = 2-t \):

When \( x=0 \), \( t=2 \); when \( x=2 \), \( t=0 \); so the limits are reversed, but the interval is the same.

\[
I = \int_{0}^{2} (2-t) \arctan(\sqrt{(2-t)(2-(2-t))}) dt
= \int_{0}^{2} (2-t) \arctan(\sqrt{t(2-t)}) dt
\]

So,

\[
I = \int_{0}^{2} x \arctan(\sqrt{x(2-x)}) dx 
= \int_{0}^{2} (2-x) \arctan(\sqrt{x(2-x)}) dx
\]

Therefore,

\[
2I = \int_{0}^{2} (x + (2-x)) \arctan(\sqrt{x(2-x)}) dx 
= \int_{0}^{2} 2 \arctan(\sqrt{x(2-x)}) dx
\]
\[
I = \int_{0}^{2} \arctan(\sqrt{x(2-x)}) dx
\]

So,
\[
\boxed{I = \int_{0}^{2} \arctan(\sqrt{x(2-x)}) dx}
\]

Now, let's compute this simpler integral.

**Step 4: Substitution for evaluation**

Let \( x = 2 \sin^2\theta \) as before, \( dx = 4\sin\theta\cos\theta d\theta = 2\sin(2\theta) d\theta \), and \( x(2-x) = 4\sin^2\theta\cos^2\theta = \sin^2(2\theta) \).

As above:

\[
I = \int_{0}^{2} \arctan(\sqrt{x(2-x)}) dx = \int_{0}^{\pi/2} \arctan(\sin(2\theta)) \cdot 4\sin\theta\cos\theta d\theta
= 2 \int_{0}^{\pi/2} \arctan(\sin(2\theta)) \sin(2\theta) d\theta
\]

Let’s make another substitution: \( \phi = 2\theta \), \( d\phi = 2 d\theta \), when \( \theta = 0 \), \( \phi = 0 \), when \( \theta = \frac{\pi}{2} \), \( \phi = \pi \).

So,

\[
I = 2 \int_{0}^{\pi/2} \arctan(\sin(2\theta)) \sin(2\theta) d\theta = \int_{0}^{\pi} \arctan(\sin\phi) \sin\phi d\phi
\]

Therefore,

\[
I = \int_{0}^{\pi} \arctan(\sin\phi) \sin\phi d\phi
\]

Now, notice that \(\arctan(\sin\phi) \) is odd about \(\phi = \pi/2\), and \( \sin\phi \) is symmetric.

But we can proceed directly.

Let’s try integrating by parts.

Let \( u = \arctan(\sin\phi) \), \( dv = \sin\phi d\phi \). Then \( du = \frac{\cos\phi}{1 + \sin^2\phi} d\phi \), and \( v = -\cos\phi \).

By parts:

\[
I = \left. -\arctan(\sin\phi)\cos\phi \right|_{\phi=0}^{\phi=\pi} + \int_{0}^{\pi} \cos\phi \cdot \frac{\cos\phi}{1 + \sin^2\phi} d\phi
\]

First term:

- \( \phi = 0 \): \( \sin(0) = 0 \), \( \arctan(0) = 0 \), \(\cos(0) = 1 \) ⇒ 0.
- \( \phi = \pi \): \( \sin(\pi) = 0 \), \( \arctan(0) = 0 \), \( \cos(\pi) = -1 \) ⇒ 0.

So, first term vanishes.

Then,

\[
I = \int_{0}^{\pi} \frac{\cos^2\phi}{1 + \sin^2\phi} d\phi
\]

Thus,
\[
I = \int_{0}^{\pi} \frac{\cos^2\phi}{1 + \sin^2\phi} d\phi
\]

Now, \( \cos^2\phi = 1 - \sin^2\phi \):

\[
I = \int_{0}^{\pi} \frac{1 - \sin^2\phi}{1 + \sin^2\phi} d\phi = \int_{0}^{\pi} \frac{1}{1 + \sin^2\phi} d\phi - \int_{0}^{\pi} \frac{\sin^2\phi}{1 + \sin^2\phi} d\phi
\]

But,

\[
\frac{\sin^2\phi}{1 + \sin^2\phi} = 1 - \frac{1}{1 + \sin^2\phi}
\]

So,

\[
I = \int_{0}^{\pi} \frac{1}{1 + \sin^2\phi} d\phi - \left[ \int_{0}^{\pi} 1 d\phi - \int_{0}^{\pi} \frac{1}{1 + \sin^2\phi}d\phi \right]
= 2\int_{0}^{\pi} \frac{1}{1 + \sin^2\phi} d\phi - \pi
\]

Thus,
\[
I = 2\int_{0}^{\pi} \frac{d\phi}{1 + \sin^2\phi} - \pi
\]

**Step 5: Evaluate the standard integral**

Let’s compute \( \int_0^\pi \frac{d\phi}{1+\sin^2\phi} \).

This is a standard integral. We recall:

\[
\int_0^\pi \frac{d\phi}{1 + k^2 \sin^2\phi} = \frac{\pi}{\sqrt{1 + k^2}}
\]

But in our case, \( k^2 = 1 \):

So,

\[
\int_0^\pi \frac{d\phi}{1 + \sin^2\phi} = \frac{\pi}{\sqrt{2}}
\]

(See tables or handbooks of definite integrals.)

**Final answer (Exact):**

\[
I = 2 \cdot \frac{\pi}{\sqrt{2}} - \pi = \pi\left(\frac{2}{\sqrt{2}} - 1\right) = \pi(\sqrt{2} - 1)
\]

**Numerical value:**

\( \sqrt{2} \approx 1.4142135624 \)

So,

\[
I \approx \pi (1.4142135624 - 1) \approx \pi \times 0.4142135624 \approx 1.3007072040
\]

Therefore:

```json
{"answer": "\\pi(\\sqrt{2}-1)", "numerical_answer": "1.3007072040"}
```