


To solve the definite integral \(\int\limits_0^1 \frac{1}{x} \arccos x \, J_1(2x) \, dx\), we proceed as follows:


### Step 1: Series Expansion of \(J_1(2x)\)
The Bessel function \(J_1(z)\) has the series expansion:
\[
J_1(z) = \sum_{n=0}^\infty \frac{(-1)^n}{n! \, (n+1)!} \left( \frac{z}{2} \right)^{2n+1}
\]
For \(z = 2x\), this becomes:
\[
J_1(2x) = \sum_{n=0}^\infty \frac{(-1)^n}{n! \, (n+1)!} x^{2n+1}
\]


### Step 2: Substitute into the Integral
The integrand \(\frac{1}{x} \arccos x \, J_1(2x)\) simplifies to:
\[
\frac{1}{x} \arccos x \, J_1(2x) = \arccos x \sum_{n=0}^\infty \frac{(-1)^n}{n! \, (n+1)!} x^{2n}
\]
Interchanging the sum and integral (justified by uniform convergence), the integral becomes:
\[
\int_0^1 \frac{1}{x} \arccos x \, J_1(2x) \, dx = \sum_{n=0}^\infty \frac{(-1)^n}{n! \, (n+1)!} \int_0^1 \arccos x \, x^{2n} \, dx
\]


### Step 3: Evaluate the Inner Integral
We compute \(\int_0^1 \arccos x \, x^{2n} \, dx\) using integration by parts. Let \(u = \arccos x\) and \(dv = x^{2n} dx\). Then \(du = -\frac{1}{\sqrt{1-x^2}} dx\) and \(v = \frac{x^{2n+1}}{2n+1}\). Applying integration by parts:
\[
\int_0^1 \arccos x \, x^{2n} \, dx = \frac{1}{2n+1} \int_0^1 \frac{x^{2n+1}}{\sqrt{1-x^2}} \, dx
\]
Using the substitution \(t = x^2\), the integral transforms into a Beta function:
\[
\int_0^1 \frac{x^{2n+1}}{\sqrt{1-x^2}} \, dx = \frac{1}{2} \int_0^1 t^n (1-t)^{-1/2} \, dt = \frac{1}{2} B\left(n+\frac{1}{2}, \frac{1}{2}\right)
\]
Using properties of the Beta function (\(B(a,b) = \frac{\Gamma(a)\Gamma(b)}{\Gamma(a+b)}\)) and Gamma function (\(\Gamma\left(n+\frac{1}{2}\right) = \frac{(2n)!\sqrt{\pi}}{4^n n!}\)), we find:
\[
\int_0^1 \arccos x \, x^{2n} \, dx = \frac{\pi \, (2n)!}{2 \, (2n+1) \, 4^n \, (n!)^2}
\]


### Step 4: Combine Terms
Substituting back, the original integral becomes:
\[
\int_0^1 \frac{1}{x} \arccos x \, J_1(2x) \, dx = \frac{\pi}{2} \sum_{n=0}^\infty \frac{(-1)^n \, (2n)!}{(n!)^3 \, (n+1) \, 4^n \, (2n+1)}
\]


### Step 5: Numerical Approximation
The series converges rapidly. Summing the first few terms gives:
\[
\sum_{n=0}^\infty \frac{(-1)^n \, 4^n}{(n+1) \, (2n+1) \, (2n+1)!} \approx 0.897315
\]


### Final Answer
The exact answer is the infinite series, and the numerical approximation is approximately \(0.897315\).

```json
{"answer": "\\frac{\\pi}{2} \\sum_{n=0}^{\\infty} \\frac{(-1)^n (2n)!}{(n!)^3 (n+1) 4^n (2n+1)}", "numerical_answer": "0.8973152904"}
```