Let's compute the integral:
\[
I = \int_0^{2\pi}\sin(\sin(x)-x)\, dx
\]

**Step 1: Analytic Calculation**

Let’s use a change of variable to examine properties.

Let \( u = 2\pi - x \), so as \( x \) goes from \( 0 \) to \( 2\pi \), \( u \) also goes from \( 2\pi \) to \( 0 \).

\( dx = -du \).

Substituting:
\[
I = \int_{x=0}^{x=2\pi} \sin(\sin(x) - x)\, dx = \int_{u=2\pi}^{u=0} \sin(\sin(2\pi-u) - (2\pi-u)) \, (-du)
\]

Since \(\sin(2\pi-u) = -\sin(u)\):

\[
\sin(\sin(2\pi-u) - (2\pi-u)) = \sin(-\sin(u) - (2\pi-u))
\]
\[
= \sin(-\sin(u) - 2\pi + u) = \sin(u - \sin(u) - 2\pi)
\]

But \(\sin(a - 2\pi) = \sin(a)\), so:
\[
= \sin(u - \sin(u))
\]

So, the integral becomes:

\[
I = \int_{u=2\pi}^{u=0} \sin(u - \sin u)\, (-du) = \int_{u=0}^{u=2\pi} \sin(u - \sin u) du
\]

But our original integral was:
\[
I = \int_0^{2\pi} \sin(\sin x - x) dx
\]
Now, note the following:

Let’s consider \( I_1 = \int_0^{2\pi} \sin(\sin x - x) dx \) \\
and \( I_2 = \int_0^{2\pi} \sin(x - \sin x) dx \)

From above, \( I_1 = I_2 \).

But notice that \( \sin(\sin x - x) = -\sin(x - \sin x) \):
\[
\sin(\sin x - x) = -\sin(x - \sin x)
\]
(because \(\sin(-A) = -\sin(A)\))

Therefore,
\[
I_1 = \int_0^{2\pi} \sin(\sin x - x) dx = -\int_0^{2\pi} \sin(x - \sin x) dx = -I_2
\]

But also, from before, \( I_1 = I_2 \).

That means \( I_1 = -I_1 \implies I_1 = 0 \).

**Step 2: Check**

Therefore, the exact value is:
\[
\int_0^{2\pi}\sin(\sin(x)-x)\, dx = 0
\]

**Step 3: Numerical Approximation**

The numerical value is \( 0.0000000000 \).

**Step 4: JSON Output**

```json
{"answer": "0", "numerical_answer": "0.0000000000"}
```