We start with the integral

  I = ∫₀¹ x·(arcsin x)·(arccos x) dx.

Step 1. Use the identity
  arcsin x + arccos x = π/2  for x ∈ [0, 1].
Thus, we can write
  arcsin x = π/2 – arccos x,
and so
  (arcsin x)(arccos x) = (π/2)·(arccos x) – (arccos x)².
Then the integral becomes
  I = (π/2)∫₀¹ x·(arccos x) dx – ∫₀¹ x·(arccos x)² dx.

Step 2. Change of variable:
Let u = arccos x. Then
  x = cos u  and  dx = –sin u du.
When x goes from 0 to 1, u goes from π/2 to 0. Reversing the integration limits, we have:

For J₁ = ∫₀¹ x·(arccos x) dx:
  J₁ = ∫₍π/2₎⁰ cos u · u · (–sin u du)
    = ∫₀^(π/2) u cos u sin u du.

For J₂ = ∫₀¹ x·(arccos x)² dx:
  J₂ = ∫₍π/2₎⁰ cos u · u² · (–sin u du)
    = ∫₀^(π/2) u² cos u sin u du.

Thus, our integral becomes
  I = (π/2)·J₁ – J₂.

Step 3. Express the sine–cosine product as:
  cos u sin u = ½ sin 2u.
Then
  J₁ = ½ ∫₀^(π/2) u sin 2u du  and  J₂ = ½ ∫₀^(π/2) u² sin 2u du.
So,
  I = (π/2)(½ ∫₀^(π/2) u sin 2u du) – ½ ∫₀^(π/2) u² sin 2u du
    = (π/4) A – (1/2) B,
where
  A = ∫₀^(π/2) u sin 2u du  and  B = ∫₀^(π/2) u² sin 2u du.

Step 4. Compute A.
Use integration by parts for A:
Let  u = u  and  dv = sin 2u du.
Then  du = du  and  v = –(cos2u)/2.
Thus,
  A = u·(–cos2u/2) – ∫ (–cos2u/2) du
    = –(u cos2u)/2 + (1/2) ∫ cos2u du.
But  ∫ cos2u du = sin2u/2.
So,
  A = –(u cos2u)/2 + (sin2u)/4.
Evaluating A from 0 to π/2:
At u = π/2: cos (π) = –1, sin (π) = 0.
  A(π/2) = –((π/2)(–1))/2 + 0 = (π/2)/2 = π/4.
At u = 0: cos 0 = 1, sin 0 = 0, hence A(0) = 0.
Thus,
  A = π/4.

Step 5. Compute B.
Again use integration by parts for B:
Let  a = u²  and  dv = sin2u du,
so that  da = 2u du  and  v = –(cos2u)/2.
Then,
  B = u² (–cos2u/2) – ∫ (–cos2u/2) (2u du)
    = –(u² cos2u)/2 + ∫ u cos2u du.
Now, compute Q = ∫ u cos2u du by parts:
Let  p = u  and  dq = cos2u du,
so that  dp = du  and  q = sin2u/2.
Then,
  Q = u (sin2u/2) – ∫ (sin2u/2) du
    = (u sin2u)/2 – (1/2) ∫ sin2u du.
Since  ∫ sin2u du = –(cos2u)/2,
we have
  Q = (u sin2u)/2 + (cos2u)/4.
Thus,
  B = –(u² cos2u)/2 + (u sin2u)/2 + (cos2u)/4.
We now evaluate B from 0 to π/2.
At u = π/2:
  cos (π) = –1, sin (π) = 0, so
  B(π/2) = –(((π/2)² (–1))/2) + 0 + ((–1))/4
       = (π²/8) – 1/4.
At u = 0:
  cos 0 = 1, sin 0 = 0, so
  B(0) = –(0) + 0 + 1/4 = 1/4.
Thus,
  B = B(π/2) – B(0) = [(π²/8) – 1/4] – (1/4) = (π²/8) – 1/2.

Step 6. Combine the results.
Recall:
  I = (π/4) A – (1/2) B.
Substitute A = π/4 and B = (π²/8) – 1/2:
  I = (π/4)(π/4) – (1/2)[(π²/8) – 1/2]
    = (π²/16) – (π²/16) + 1/4
    = 1/4.

Step 7. Numerical approximation:
  1/4 = 0.25, which to 10 decimal places is 0.2500000000.

Thus, the final answer is:

{"answer": "\\frac{1}{4}", "numerical_answer": "0.2500000000"}