Let's denote the integral as
\[
I = \int_{1/\sqrt{2}}^1 \frac{\arcsin(x)}{x^3} \, dx.
\]

## Step 1: Compute the indefinite integral

We use integration by parts:
Let \( u = \arcsin(x) \), \( dv = x^{-3} dx \).

Then,
\[
du = \frac{1}{\sqrt{1 - x^2}} dx, \quad v = -\frac{1}{2} x^{-2}
\]

Integration by parts formula:
\[
\int u \, dv = uv - \int v \, du
\]

So,
\[
\int \frac{\arcsin(x)}{x^3} dx = \arcsin(x) \cdot \left(-\frac{1}{2} x^{-2}\right) - \int \left(-\frac{1}{2} x^{-2}\right) \cdot \frac{1}{\sqrt{1-x^2}} dx
\]
\[
= -\frac{\arcsin(x)}{2x^2} + \frac{1}{2} \int \frac{1}{x^2 \sqrt{1-x^2}} dx
\]

Now, let's handle \(\int \frac{1}{x^2 \sqrt{1-x^2}} dx\).

Let us write the integrand:
\[
\frac{1}{x^2 \sqrt{1-x^2}}
\]

Letâ€™s make the substitution \( x = \sin \theta \), so \( dx = \cos\theta d\theta \). Then,

\[
\frac{1}{x^2 \sqrt{1-x^2}} dx = \frac{1}{\sin^2\theta \cdot \cos\theta} \cos\theta d\theta = \frac{1}{\sin^2\theta} d\theta = \csc^2\theta d\theta
\]

Also, \( \arcsin(x) = \theta \), so our indefinite integral is:
\[
-\frac{\theta}{2\sin^2\theta} + \frac{1}{2} \int \csc^2\theta d\theta
\]
\[
= -\frac{\arcsin(x)}{2x^2} - \frac{1}{2} \cot\theta + C
\]
Note that \(\int \csc^2\theta d\theta = -\cot\theta\), and \(\cot\theta = \sqrt{1-x^2}/x\).

So,
\[
\int \frac{\arcsin(x)}{x^3} dx = -\frac{\arcsin(x)}{2x^2} - \frac{1}{2} \cdot \frac{\sqrt{1-x^2}}{x} + C
\]

## Step 2: Evaluate the definite integral

Plug in the limits:

\[
I = F(1) - F\left(\frac{1}{\sqrt{2}}\right)
\]
where
\[
F(x) = -\frac{\arcsin(x)}{2x^2} - \frac{1}{2} \cdot \frac{\sqrt{1-x^2}}{x}
\]

**At** \(x = 1\): 
\[
\arcsin(1) = \frac{\pi}{2}, \quad \sqrt{1-1^2} = 0
\]
\[
F(1) = -\frac{\pi/2}{2 \cdot 1^2} - \frac{1}{2} \cdot 0 = -\frac{\pi}{4}
\]

**At** \(x = 1/\sqrt{2}\):
\[
\arcsin(1/\sqrt{2}) = \arcsin(\sqrt{2}/2) = \frac{\pi}{4}
\]
\[
\sqrt{1 - (1/\sqrt{2})^2} = \sqrt{1 - 1/2} = \sqrt{1/2} = \frac{1}{\sqrt{2}}
\]
\[
\frac{\sqrt{1-x^2}}{x} = \frac{1/\sqrt{2}}{1/\sqrt{2}} = 1
\]

\[
x^2 = (1/\sqrt{2})^2 = 1/2
\]
So,
\[
-\frac{\arcsin(x)}{2x^2} = -\frac{\pi/4}{2 \cdot (1/2)} = -\frac{\pi/4}{1} = -\frac{\pi}{4}
\]
\[
-\frac{1}{2} \cdot 1 = -\frac{1}{2}
\]

\[
F(1/\sqrt{2}) = -\frac{\pi}{4} - \frac{1}{2}
\]

So, the definite integral:
\[
I = F(1) - F(1/\sqrt{2}) = \left( -\frac{\pi}{4} \right) - \left( -\frac{\pi}{4} - \frac{1}{2} \right)
= -\frac{\pi}{4} + \frac{\pi}{4} + \frac{1}{2} 
= \frac{1}{2}
\]

## Step 3: Numerical approximation

\[
\frac{1}{2} = 0.5
\]

## Step 4: JSON output

```json
{"answer": "\\frac{1}{2}", "numerical_answer": "0.5"}
```