Given:
\[
\int_0^{2.0} x^{-1.0/4} (2.0 - x)^{-(1.0+2)/4} I_{1.0}\left(1.0 \sqrt[4]{x(2.0-x)}\right)\, dx
\]
which simplifies the exponents:
\[
\int_0^{2} x^{-1/4} (2-x)^{-3/4} I_1\left((x(2-x))^{1/4}\right)\, dx
\]

Let’s proceed step by step:

---

### **Step 1: Change of Variables**

Set \( x = 2t \), with \( t \in [0, 1] \), so \( dx = 2dt \):
- \( x^{-1/4} = (2t)^{-1/4} = 2^{-1/4} t^{-1/4} \)
- \( 2 - x = 2 - 2t = 2(1-t) \implies (2-x)^{-3/4} = 2^{-3/4} (1-t)^{-3/4} \)
- \( x(2-x) = 2t \times 2(1-t) = 4t(1-t) \implies (x(2-x))^{1/4} = (4t(1-t))^{1/4} = 2^{1/2} (t(1-t))^{1/4} \)

Substituting all together:
\[
\begin{align*}
&\int_0^{2} x^{-1/4} (2-x)^{-3/4} I_1\left((x(2-x))^{1/4}\right)\, dx \\
=~ & \int_{t=0}^1 2^{-1/4} t^{-1/4} ~ 2^{-3/4} (1-t)^{-3/4} ~ I_1\left(2^{1/2} (t(1-t))^{1/4}\right) \times 2 dt \\
=~ & 2^{1 - 1/4 - 3/4} \int_0^1 t^{-1/4} (1-t)^{-3/4} I_1\left(2^{1/2}(t(1-t))^{1/4}\right) dt \\
=~ & 2^{0} \int_0^1 t^{-1/4} (1-t)^{-3/4} I_1\left(2^{1/2}(t(1-t))^{1/4}\right) dt \\
=~ & \int_0^1 t^{-1/4} (1-t)^{-3/4} I_1\left(\sqrt{2}(t(1-t))^{1/4}\right) dt
\end{align*}
\]

---

### **Step 2: Analytical Evaluation of the Integral**

Let’s recall the integral involving the Bessel function:
\[
\int_0^1 t^{c-1} (1-t)^{d-c-1} I_\nu\left(2 a t^{1/2}(1-t)^{1/2}\right) dt
\]
has the solution:
\[
\frac{\Gamma(c)\Gamma(d-c)}{\Gamma(d)} {}_1F_1\left(\nu + c; d; a^2\right) \cdot \frac{a^\nu}{2^\nu \Gamma(\nu+1)}
\]
(*from Gradshteyn & Ryzhik 6.643.2, with \( b = 1 \), \( t \to t \), \( x = t \), limits 0 to 1*)

Let’s adjust to our case:
* Our exponent on \( t \) is \(-1/4 = c-1 \implies c = 3/4 \).
* Exponent on \( 1-t \) is \(-3/4 = d-c-1 \implies d-c = 1/4 \implies d = c + 1/4 = 1 \).
* So \( d = 1 \).
* Our \( \nu = 1 \).
* Argument is \( \sqrt{2} (t(1-t))^{1/4} = \sqrt{2} \cdot \left(t(1-t)\right)^{1/4} \).

But the formula in G&R is for \( I_\nu(2a \sqrt{t(1-t)}) \). We have \( I_1\left(\sqrt{2}[t(1-t)]^{1/4}\right) \). The arguments do not exactly match.

Let’s try a substitution to match the form in G&R.

#### Let’s try \( u = \sqrt[4]{t(1-t)} \), but more effective is to look for a standard form if any.

#### Alternatively, note that the integral is closely related to the Laplace transform of Bessel functions or hypergeometric or beta integrals.

#### Let’s recall the Series Expansion for \( I_1(x) \):
\[
I_1(x) = \sum_{n=0}^\infty \frac{1}{n! \Gamma(n+2)} \left(\frac{x}{2}\right)^{2n+1}
\]

Let’s plug this into the integral:
\[
\int_0^{1} t^{-1/4} (1-t)^{-3/4} \sum_{n=0}^\infty \frac{1}{n! \Gamma(n+2)} \left( \frac{\sqrt{2}(t(1-t))^{1/4}}{2} \right)^{2n+1} dt
\]
Interchange sum and integral (justified for positive integrand and absolute convergence):

\[
\sum_{n=0}^\infty \frac{(\sqrt{2}/2)^{2n+1}}{n! \Gamma(n+2)} \int_0^1 t^{-1/4+(2n+1)/4} (1-t)^{-3/4+(2n+1)/4} dt
\]

\[
= \sum_{n=0}^\infty \frac{2^{(2n+1)/2} 2^{-(2n+1)}}{n! \Gamma(n+2)} 
\int_0^1 t^{(2n+1-1)/4} (1-t)^{(2n+1-3)/4} dt
\]

But let's compute the exponents in the integral:
- For \( t \): \( -1/4 + (2n+1)/4 = (2n+1-1)/4 = (2n)/4 = n/2 \)
- For \( 1-t \): \( -3/4 + (2n+1)/4 = (2n+1-3)/4 = (2n-2)/4 = (n-1)/2 \)

So, the integral becomes (which is a Beta function):

\[
\int_0^1 t^{n/2} (1-t)^{(n-1)/2} dt = \mathrm{B}(n/2 + 1, (n-1)/2 + 1) = \frac{\Gamma(n/2+1) \Gamma((n+1)/2)}{\Gamma(n+3/2)}
\]

Now, let's combine all constants.
- \( (\sqrt{2}/2)^{2n+1} = 2^{(2n+1)/2 - (2n+1)} = 2^{(2n+1)(1/2-1)} = 2^{-(2n+1)/2} \)
- But let's write as \( 2^{- (2n+1)/2} \)

So, the sum is:
\[
\sum_{n=0}^\infty \frac{2^{-(2n+1)/2}}{n! \Gamma(n+2)} \frac{\Gamma(n/2+1) \Gamma((n+1)/2)}{\Gamma(n+3/2)}
\]

### Let's try to further simplify that expression

But let's instead check for a known result in the book or in standard integrals.

#### Alternatively, let's check Wolfram function references.

But it's not matching a standard integral, so the sum formula is as far as we get analytically.

---

### **Step 3: Final Analytical Answer**

Thus, the exact analytical value is:
\[
\boxed{
\int_0^2 x^{-1/4} (2-x)^{-3/4} I_1\left((x(2-x))^{1/4}\right)\, dx = \sum_{n=0}^{\infty} \frac{2^{-(2n+1)/2}}{n!\, \Gamma(n+2)} \cdot \frac{\Gamma(n/2+1)\, \Gamma\left(\frac{n+1}{2}\right)}{\Gamma(n+3/2)}
}
\]
or, equivalently,
\[
\boxed{
\int_0^2 x^{-1/4} (2-x)^{-3/4} I_1\left((x(2-x))^{1/4}\right)\, dx =
\sum_{n=0}^{\infty}
\frac{2^{-(2n+1)/2} \, \Gamma(n/2+1)\, \Gamma((n+1)/2)}
     {n! \, \Gamma(n+2)\, \Gamma(n+3/2)}
}
\]

---

### **Step 4: Numerical Value**

Let’s compute the first few terms of the series:

Let’s write in code notation for the sum:

For \( n = 0 \):
- \( n! = 1 \), \( \Gamma(n+2) = 1! = 1 \), \( \Gamma(n/2+1) = \Gamma(1) = 1 \), \( \Gamma((n+1)/2) = \Gamma(0.5) = \sqrt{\pi} \), \( \Gamma(n+3/2) = \Gamma(1.5) = 0.5 \sqrt{\pi} \), \( 2^{-(2n+1)/2} = 2^{-1/2} = 1/\sqrt{2} \)
- So, first term: \( \frac{1}{\sqrt{2}} \cdot \frac{1 \cdot \sqrt{\pi}}{1 \cdot 1 \cdot 0.5\sqrt{\pi}} = \frac{1}{\sqrt{2}} \cdot \frac{2}{1} = \frac{2}{\sqrt{2}} = \sqrt{2} \approx 1.414213562 \)

For \( n = 1 \):
- \( n! = 1 \), \( \Gamma(n+2) = \Gamma(3) = 2 \), \( \Gamma(1/2+1) = \Gamma(1.5) = 0.5 \sqrt{\pi} \), \( \Gamma(1) = 1 \), \( \Gamma(2.5) \)
- \( 2^{-(3)/2} = 2^{-1.5} = 1/(2 \sqrt{2}) = 0.3535533906 \)
- \( \Gamma(2.5) = (3/2)\Gamma(1.5) = (3/2) \times 0.5\sqrt{\pi} = 0.75 \sqrt{\pi} \)
So,
\[
0.3535533906 \cdot \frac{0.5\sqrt{\pi} \cdot 1}{1 \cdot 2 \cdot 0.75\sqrt{\pi}} = 0.3535533906 \cdot \frac{0.5}{1.5} = 0.3535533906 \cdot 0.3333333 = 0.1178511302
\]

For \( n = 2 \):
- \( n! = 2 \), \( \Gamma(4) = 6 \), \( \Gamma(2) = 1 \), \( \Gamma(1.5) = 0.5\sqrt{\pi} \), \( \Gamma(3.5) \)
- \( 2^{-(5)/2} = 2^{-2.5} = 1/(4 \sqrt{2}) = 0.1767766953 \)
- \( \Gamma(3.5) = (5/2)\Gamma(2.5) = (2.5)\times 0.75\sqrt{\pi} = 1.875\sqrt{\pi} \)
So,
\[
0.1767766953 \cdot \frac{1 \cdot 0.5\sqrt{\pi}}{2 \cdot 6 \cdot 1.875\sqrt{\pi}} = 0.1767766953 \cdot \frac{0.5}{22.5} = 0.1767766953 \cdot 0.0222222 = 0.0039505932
\]

For \( n = 3 \):
- \( n! = 6 \), \( \Gamma(5) = 24 \), \( \Gamma(2.5) = 0.75 \sqrt{\pi} \), \( \Gamma(2) = 1 \), \( \Gamma(4.5) \)
- \( 2^{-7/2} = 2^{-3.5} = 1/(8 \sqrt{2}) = 0.08838834765 \)
- \( \Gamma(4.5) = (7/2)\Gamma(3.5) = 3.5 \times 1.875\sqrt{\pi} = 6.5625\sqrt{\pi} \)
So,
\[
0.08838834765 \cdot \frac{0.75\sqrt{\pi} \cdot 1}{6 \cdot 24 \cdot 6.5625\sqrt{\pi}} =
0.08838834765 \cdot \frac{0.75}{945} = 0.08838834765 \cdot 0.00079365 = 0.0000701828
\]

The terms decrease rapidly. Summing the first 4:

- \( 1.414213562 + 0.1178511302 + 0.0039505932 + 0.0000701828 = 1.5360854682 \)

Continue for a few more terms, but the sum converges quickly.

For \( n=4 \):
- \( n! = 24 \), \( \Gamma(6) = 120 \), \( \Gamma(3) = 2 \), \( \Gamma(2.5) = 0.75\sqrt{\pi} \), \( \Gamma(5.5) \)
- \( 2^{-9/2} = 2^{-4.5} = 1/(16\sqrt{2}) = 0.04419417382 \)
- \( \Gamma(5.5) = (9/2)\Gamma(4.5) = 4.5 \times 6.5625\sqrt{\pi} = 29.53125\sqrt{\pi} \)
Calculate inner numerator: \( 2 \times 0.75 \sqrt{\pi} = 1.5\sqrt{\pi} \)
Denominator: \( 24 \times 120 \times 29.53125\sqrt{\pi} = 24 \times 120 = 2880 \), \( 2880 \times 29.53125 = 85049.16 \)
So \( 85049.16 \sqrt{\pi} \)
So,
\[
0.04419417382 \times \frac{1.5}{85049.16} = 0.04419417382 \cdot 0.000017641 = 0.0000007796
\]
So adding, it becomes \( 1.5360862478 \).

The later terms are negligible at the 10th decimal.

Therefore, the numerical approximation is:
\[
1.5360862478
\]

---

## **Final JSON Answer**

```json
{"answer": "\\displaystyle \\sum_{n=0}^{\\infty} \\frac{2^{-(2n+1)/2} \\, \\Gamma(n/2+1)\\, \\Gamma((n+1)/2)}{n!\\, \\Gamma(n+2)\\, \\Gamma(n+3/2)}", "numerical_answer": "1.5360862478"}
```