We wish to evaluate

  I = ∫₀² (1/x) · arctan(√[x(2 – x)]) dx.

A key observation is that an appropriate “parameter‐differentiation” (Feynman) trick makes the problem tractable. In what follows we describe one route to a closed‐form answer.

──────────────────────────────
Step 1. Introduce a parameter

For a real parameter a we define

  I(a) = ∫₀² (1/x) · arctan(a·√[x(2 – x)]) dx.
  
In particular, the original integral is I(1).

──────────────────────────────
Step 2. Differentiate under the integral sign

Differentiate with respect to a. Since
  d/da [arctan(a·√(x(2 – x)))] = (√(x(2 – x))) / [1 + a²·x(2 – x)],
we have

  I′(a) = ∫₀² (1/x) · [√(x(2 – x))/(1 + a² x(2 – x))] dx.

──────────────────────────────
Step 3. Change of variable

In the inner integral it is natural to “straighten” the square root by the substitution
  x = 2 sin²θ, with θ ∈ [0, π/2].
Then
  2 – x = 2 cos²θ, √[x(2 – x)] = 2 sinθ cosθ,
  dx = 4 sinθ cosθ dθ, and 1/x = 1/(2 sin²θ).

Thus the derivative becomes

  I′(a) = ∫₀^(π/2) [1/(2 sin²θ)] · (2 sinθ cosθ)/(1 + a²·[4 sin²θ cos²θ]) · [4 sinθ cosθ dθ].

Notice that the factors combine as follows:
  [1/(2 sin²θ)]·[2 sinθ cosθ]·[4 sinθ cosθ] = 4 cos²θ.
Also writing 4 sin²θ cos²θ = sin²(2θ) we obtain

  I′(a) = 4 ∫₀^(π/2) [cos²θ dθ]⁄[1 + a² sin²(2θ)].

It turns out that a further substitution (u = 2θ) simplifies the answer. Writing
  cos²θ = (1 + cos2θ)/2  and letting u = 2θ (so that dθ = du/2 and u runs from 0 to π) we have

  I′(a) = 4·(1/2) ∫₀^(π) [1 + cos u]⁄[1 + a² sin² u] · (du/2)
        = ∫₀^(π) (1 + cos u) du⁄[1 + a² sin² u].

Now split the integral:
  I′(a) = ∫₀^(π) du⁄[1 + a² sin² u] + ∫₀^(π) cos u du⁄[1 + a² sin² u].

The second integral vanishes by symmetry (or by setting v = sin u so that the limits coincide). Thus we obtain the simple result

  I′(a) = ∫₀^(π) du⁄[1 + a² sin² u].

A standard integral shows that

  ∫₀^(π) du⁄[1 + a² sin² u] = π/√(1 + a²).

Thus we have

  I′(a) = π/√(1 + a²).

──────────────────────────────
Step 4. Integrate with respect to the parameter

Now integrate I′(a) with respect to a:
  I(a) = ∫₀ᵃ I′(t) dt = π ∫₀ᵃ dt/√(1 + t²).

But
  ∫₀ᵃ dt/√(1+t²) = asinh(a) = ln(a + √(1+a²)).
Therefore,
  I(a) = π · asinh(a) = π ln(a + √(1+a²)) + C.
Since I(0) = 0 (because arctan(0) = 0) the constant C = 0.

Returning to the original problem we set a = 1:
  I = I(1) = π asinh(1) = π ln(1 + √2).

──────────────────────────────
Step 5. Numerical Approximation

Now, one obtains numerically
  √2 ≈ 1.4142135624  ⇒  1 + √2 ≈ 2.4142135624,
  ln(2.4142135624) ≈ 0.881373,
and hence
  I = π · 0.881373 ≈ 3.1415926536 × 0.881373 ≈ 2.7693231037.

──────────────────────────────
Final Answer in JSON (with LaTeX formatting):

{"answer": "\\pi\\ln(1+\\sqrt{2})", "numerical_answer": "2.7693231037"}