Let's compute the definite integral:
\[
I = \int_0^\pi \cos(x + \cos x)\,dx
\]

**Step 1: Use a substitution to simplify the integral.**

Let us consider the substitution \( u = \pi - x \), so as \( x \) goes from \( 0 \) to \( \pi \), \( u \) also goes from \( \pi \) to \( 0 \). Let's carefully compute the transformed integral:

\[
I = \int_{x=0}^{x=\pi} \cos(x + \cos x)\,dx
\]

Let \( u = \pi - x \implies x = \pi - u, dx = -du \)

So when \( x=0 \), \( u=\pi \) and when \( x=\pi \), \( u=0 \):

\[
I = \int_{u=\pi}^{u=0} \cos((\pi-u) + \cos(\pi-u)) \cdot (-du)
\]
\[
= \int_{u=0}^{u=\pi} \cos((\pi-u) + \cos(\pi-u)) du
\]

Recall that \( \cos(\pi-u) = -\cos u \), so:

\[
(\pi-u) + \cos(\pi-u) = (\pi-u) + (-\cos u) = \pi - u - \cos u
\]

Thus our integral becomes:

\[
I = \int_{0}^{\pi} \cos(\pi - u - \cos u) \, du
\]

But \( \cos(\pi - A) = -\cos A \), so:

\[
\cos(\pi - u - \cos u) = -\cos(u + \cos u)
\]

Therefore,
\[
I = \int_0^{\pi} -\cos(u + \cos u) du = -I
\]

So,
\[
I = -I \implies 2I = 0 \implies I = 0
\]

**Step 2: All necessary steps have been provided above, using symmetry.**

**Step 3: Numerical approximation**

The result is exactly zero, so the approximate value is \(0.0000000000\).

**Step 4: Output in JSON format**

```json
{"answer": "0", "numerical_answer": "0.0000000000"}
```