<think>
Okay, so I need to compute the definite integral from 0 to π/2 of [sin^{2n}x / (sin^{2n}x + cos^{2n}x)] dx. Hmm, let's see. I remember that integrals over 0 to π/2 sometimes have symmetry properties that can be exploited. Maybe substitution? Let me think.

First, when I see the limits from 0 to π/2 and the integrand involving sin and cos, a common technique is to use the substitution x = π/2 - t. Let me try that. If I let t = π/2 - x, then when x is 0, t is π/2, and when x is π/2, t is 0. The differential dx becomes -dt, but since we reverse the limits, the integral becomes the same as integrating from 0 to π/2. So, substituting, the integral becomes:

I = ∫₀^{π/2} [sin^{2n}(π/2 - t) / (sin^{2n}(π/2 - t) + cos^{2n}(π/2 - t))] dt

But sin(π/2 - t) is cos t, and cos(π/2 - t) is sin t. So substituting those in:

I = ∫₀^{π/2} [cos^{2n}t / (cos^{2n}t + sin^{2n}t)] dt

Wait, the original integral was [sin^{2n}x / (sin^{2n}x + cos^{2n}x)] dx, and after substitution, it's [cos^{2n}t / (cos^{2n}t + sin^{2n}t)] dt. So if I call the original integral I, then after substitution, I get another integral which is similar but with cos in the numerator. Let me denote the original integral as I. Then, after substitution, I have:

I = ∫₀^{π/2} [cos^{2n}t / (cos^{2n}t + sin^{2n}t)] dt

But notice that if I add the original integral and this substituted integral, I get:

I + I = ∫₀^{π/2} [sin^{2n}x / (sin^{2n}x + cos^{2n}x) + cos^{2n}x / (sin^{2n}x + cos^{2n}x)] dx

Which simplifies to:

2I = ∫₀^{π/2} [ (sin^{2n}x + cos^{2n}x) / (sin^{2n}x + cos^{2n}x) ] dx = ∫₀^{π/2} 1 dx = π/2

Therefore, 2I = π/2, so I = π/4. Wait, that seems too straightforward. But does this hold for any n? Let me check for n=1. If n=1, the integrand becomes sin²x / (sin²x + cos²x) = sin²x, since sin²x + cos²x =1. Then the integral from 0 to π/2 of sin²x dx. The integral of sin²x is (x - sinx cosx)/2 evaluated from 0 to π/2. At π/2, sinx=1, cosx=0, so (π/2 - 0)/2 = π/4. At 0, it's 0. So the integral is π/4. Which matches the result I just found. So for n=1, it works. What about n=2? Let's see. The integrand would be sin^4x / (sin^4x + cos^4x). Hmm, integrating that from 0 to π/2. If I use the same substitution, then adding the two integrals would give π/2, so each integral is π/4. So even for n=2, the integral is π/4. Wait, so is this integral always π/4 regardless of n? That seems surprising, but the substitution trick shows that. Because when you substitute x = π/2 - t, you get the same form but with cos and sin swapped, and adding them gives the integral of 1 over the interval, which is π/2. Therefore, each integral must be half of that, so π/4. Therefore, the answer is π/4 for any n.

But let me check another case. Let n=0. Then the integrand becomes 1/(1+1) = 1/2, so the integral is (π/2)*(1/2) = π/4. Which still holds. So even n=0, which is a trivial case, gives π/4. So this seems to hold for all n. Therefore, the integral is π/4. So the exact answer is π/4, and the numerical approximation is approximately 0.7853981634. Rounded to 10 decimal places, that's 0.7853981634. Let me confirm with another approach. Suppose I let t = tan x. Then x = arctan t, dx = dt/(1 + t²). The limits when x=0, t=0; x=π/2, t approaches infinity. Then the integral becomes:

∫₀^∞ [ (t^{2n}/(1 + t²)^{n}) / (t^{2n}/(1 + t²)^{n} + 1/(1 + t²)^{n}) ) ] * (dt/(1 + t²))

Simplify the integrand:

The numerator is t^{2n}/(1 + t²)^n, denominator is [t^{2n} + 1]/(1 + t²)^n. So the fraction simplifies to t^{2n}/(t^{2n} + 1). Then the integral becomes ∫₀^∞ [t^{2n}/(t^{2n} + 1)] * [1/(1 + t²)] dt.

Hmm, not sure if that helps. But maybe using substitution here. Let me set u = 1/t. Then when t approaches 0, u approaches infinity, and vice versa. The integral becomes:

∫₀^∞ [t^{2n}/(t^{2n} + 1)] * [1/(1 + t²)] dt = ∫₀^∞ [ (1/u^{2n}) / (1/u^{2n} + 1) ) ] * [1/(1 + 1/u²)] * ( -1/u² du )

But the negative sign is canceled by swapping the integral limits, so it becomes:

∫₀^∞ [1/(1 + u^{2n})] * [u²/(1 + u²)] * (1/u²) du = ∫₀^∞ [1/(1 + u^{2n})] * [1/(1 + u²)] du

But that's the same as the original integral. So adding the original integral and this substitution, we get:

I = ∫₀^∞ [t^{2n}/(t^{2n} + 1) + 1/(1 + t^{2n})] * [1/(1 + t²)] dt / 2

Wait, but the sum inside the brackets is [ (t^{2n} + 1)/(t^{2n} + 1) ] = 1. So the integral becomes (1/2) ∫₀^∞ [1/(1 + t²)] dt = (1/2)*(π/2) = π/4. So again, we get I = π/4. Therefore, this confirms the result. So regardless of the approach, the integral is π/4. Therefore, the exact answer is π/4, and the numerical approximation is approximately 0.7853981634.
</think>

{"answer": "\\frac{\\pi}{4}", "numerical_answer": 0.7853981634}