

To solve the definite integral \(\int\limits_0^{2} x^{1/2}(2 - x)^{-1/2}\cos\left(\sqrt{x(2 - x)}\right)dx\), we proceed with the following steps:

### Step 1: Substitution to Simplify the Integral
Let \( t = \frac{x}{2} \), so \( x = 2t \), \( dx = 2dt \), and the limits change from \( x = 0 \) to \( t = 0 \) and \( x = 2 \) to \( t = 1 \). Substituting into the integral:
\[
\sqrt{x} = \sqrt{2t} = \sqrt{2}\sqrt{t}, \quad \sqrt{2 - x} = \sqrt{2(1 - t)} = \sqrt{2}\sqrt{1 - t}
\]
Thus, \( \frac{\sqrt{x}}{\sqrt{2 - x}} = \sqrt{\frac{t}{1 - t}} \). The argument of the cosine becomes:
\[
\sqrt{x(2 - x)} = \sqrt{2t \cdot 2(1 - t)} = 2\sqrt{t(1 - t)}
\]
The integral transforms to:
\[
\int_0^1 \sqrt{\frac{t}{1 - t}} \cos\left(2\sqrt{t(1 - t)}\right) \cdot 2dt = 2\int_0^1 \sqrt{\frac{t}{1 - t}} \cos\left(2\sqrt{t(1 - t)}\right) dt
\]

### Step 2: Trigonometric Substitution
Let \( t = \sin^2\theta \), so \( dt = 2\sin\theta\cos\theta d\theta \), and \( \theta \) ranges from \( 0 \) to \( \frac{\pi}{2} \). Then:
\[
\sqrt{\frac{t}{1 - t}} = \tan\theta, \quad \sqrt{t(1 - t)} = \sin\theta\cos\theta
\]
The argument of the cosine becomes \( 2\sin\theta\cos\theta = \sin(2\theta) \). Substituting these into the integral:
\[
2\int_0^{\pi/2} \tan\theta \cdot \cos(\sin(2\theta)) \cdot 2\sin\theta\cos\theta d\theta = 4\int_0^{\pi/2} \sin^2\theta \cos(\sin(2\theta)) d\theta
\]

### Step 3: Further Simplification
Let \( \phi = 2\theta \), so \( \theta = \frac{\phi}{2} \), \( d\theta = \frac{d\phi}{2} \), and \( \phi \) ranges from \( 0 \) to \( \pi \). Then \( \sin^2\theta = \frac{1 - \cos\phi}{2} \), and the integral becomes:
\[
4\int_0^{\pi} \frac{1 - \cos\phi}{2} \cos(\sin\phi) \cdot \frac{d\phi}{2} = \int_0^{\pi} (1 - \cos\phi)\cos(\sin\phi) d\phi
\]

### Step 4: Evaluating the Integral
Split the integral into two parts:
\[
\int_0^{\pi} \cos(\sin\phi) d\phi - \int_0^{\pi} \cos\phi\cos(\sin\phi) d\phi
\]
- The first integral \( \int_0^{\pi} \cos(\sin\phi) d\phi \) is a known result related to Bessel functions. For \( J_0(z) \) (the Bessel function of the first kind of order 0), we have:
  \[
  J_0(z) = \frac{1}{\pi}\int_0^{\pi} \cos(z\sin\phi) d\phi
  \]
  Setting \( z = 1 \), we get \( \int_0^{\pi} \cos(\sin\phi) d\phi = \pi J_0(1) \).

- The second integral \( \int_0^{\pi} \cos\phi\cos(\sin\phi) d\phi \) simplifies using the substitution \( t = \sin\phi \), \( dt = \cos\phi d\phi \). The limits \( \phi = 0 \) to \( \phi = \pi \) map to \( t = 0 \) to \( t = 0 \), so the integral is \( 0 \).

### Final Result
The original integral simplifies to \( \pi J_0(1) \).

### Numerical Approximation
The Bessel function \( J_0(1) \approx 0.7651976865579666 \). Thus:
\[
\pi J_0(1) \approx 3.141592653589793 \times 0.7651976865579666 \approx 2.4039340881
\]

{"answer": "\(\pi J_0(1)\)", "numerical_answer": "2.4039340881"}