To solve the definite integral 

\[
\int_0^{\frac{\pi}{4}} \tan^{-1}\left(\frac{1 + \tan(x)}{\sqrt{2}}\right) \mathrm{d}x,
\]

we will proceed with the following steps:

### Step 1: Substitution
Let’s make the substitution \( u = \tan(x) \). Then, \( \mathrm{d}u = \sec^2(x) \mathrm{d}x \), and the limits change as follows:
- When \( x = 0 \), \( u = 0 \).
- When \( x = \frac{\pi}{4} \), \( u = 1 \).

The integral becomes:

\[
\int_{0}^{1} \tan^{-1}\left(\frac{1 + u}{\sqrt{2}}\right) \frac{\mathrm{d}u}{1 + u^2}.
\]

### Step 2: Integration by Parts
Let’s denote:

\[
I = \int_{0}^{1} \tan^{-1}\left(\frac{1 + u}{\sqrt{2}}\right) \frac{\mathrm{d}u}{1 + u^2}.
\]

We can use integration by parts with:
- \( v = \tan^{-1}\left(\frac{1 + u}{\sqrt{2}}\right) \), so \( \mathrm{d}v = \frac{1}{1 + \left(\frac{1 + u}{\sqrt{2}}\right)^2} \cdot \frac{1}{\sqrt{2}} \mathrm{d}u = \frac{\sqrt{2}}{2 + (1 + u)^2} \mathrm{d}u \).
- \( \mathrm{d}w = \frac{\mathrm{d}u}{1 + u^2} \), so \( w = \tan^{-1}(u) \).

Applying integration by parts:

\[
I = \left. \tan^{-1}(u) \tan^{-1}\left(\frac{1 + u}{\sqrt{2}}\right) \right|_{0}^{1} - \int_{0}^{1} \tan^{-1}(u) \cdot \frac{\sqrt{2}}{2 + (1 + u)^2} \mathrm{d}u.
\]

Evaluating the boundary term:

\[
\left. \tan^{-1}(u) \tan^{-1}\left(\frac{1 + u}{\sqrt{2}}\right) \right|_{0}^{1} = \tan^{-1}(1) \tan^{-1}\left(\frac{2}{\sqrt{2}}\right) - 0 = \frac{\pi}{4} \cdot \tan^{-1}(\sqrt{2}).
\]

Now, let’s denote the remaining integral as \( J \):

\[
J = \int_{0}^{1} \tan^{-1}(u) \cdot \frac{\sqrt{2}}{2 + (1 + u)^2} \mathrm{d}u.
\]

### Step 3: Simplifying \( J \)
We can rewrite \( J \) as:

\[
J = \sqrt{2} \int_{0}^{1} \frac{\tan^{-1}(u)}{2 + (1 + u)^2} \mathrm{d}u.
\]

This integral is complex, but we can observe that the original integral \( I \) can be approached differently. Instead, let’s consider the derivative of \( \tan^{-1}\left(\frac{1 + \tan(x)}{\sqrt{2}}\right) \):

\[
\frac{\mathrm{d}}{\mathrm{d}x} \tan^{-1}\left(\frac{1 + \tan(x)}{\sqrt{2}}\right) = \frac{\sec^2(x)}{\sqrt{2} \left(1 + \left(\frac{1 + \tan(x)}{\sqrt{2}}\right)^2\right)} = \frac{\sec^2(x)}{\sqrt{2} \left(1 + \frac{(1 + \tan(x))^2}{2}\right)}.
\]

Simplifying the denominator:

\[
1 + \frac{(1 + \tan(x))^2}{2} = \frac{2 + (1 + \tan(x))^2}{2} = \frac{3 + 2\tan(x) + \tan^2(x)}{2}.
\]

Thus:

\[
\frac{\mathrm{d}}{\mathrm{d}x} \tan^{-1}\left(\frac{1 + \tan(x)}{\sqrt{2}}\right) = \frac{\sec^2(x)}{\sqrt{2}} \cdot \frac{2}{3 + 2\tan(x) + \tan^2(x)} = \frac{2 \sec^2(x)}{\sqrt{2} (3 + 2\tan(x) + \tan^2(x))}.
\]

This suggests that the integral might not simplify easily via differentiation. Instead, let’s consider an alternative approach by recognizing that:

\[
\tan^{-1}\left(\frac{1 + \tan(x)}{\sqrt{2}}\right) = \tan^{-1}\left(\frac{1}{\sqrt{2}}\right) + \tan^{-1}\left(\frac{\tan(x)}{\sqrt{2} + 1}\right).
\]

However, this identity does not hold generally, so we must abandon this path.

### Step 4: Alternative Approach
Let’s consider the integral:

\[
I = \int_{0}^{\frac{\pi}{4}} \tan^{-1}\left(\frac{1 + \tan(x)}{\sqrt{2}}\right) \mathrm{d}x.
\]

We can use the substitution \( x = \frac{\pi}{4} - t \), so \( \mathrm{d}x = -\mathrm{d}t \), and the limits change as follows:
- When \( x = 0 \), \( t = \frac{\pi}{4} \).
- When \( x = \frac{\pi}{4} \), \( t = 0 \).

The integral becomes:

\[
I = \int_{0}^{\frac{\pi}{4}} \tan^{-1}\left(\frac{1 + \tan\left(\frac{\pi}{4} - t\right)}{\sqrt{2}}\right) \mathrm{d}t.
\]

Using the identity \( \tan\left(\frac{\pi}{4} - t\right) = \frac{1 - \tan(t)}{1 + \tan(t)} \), we have:

\[
I = \int_{0}^{\frac{\pi}{4}} \tan^{-1}\left(\frac{1 + \frac{1 - \tan(t)}{1 + \tan(t)}}{\sqrt{2}}\right) \mathrm{d}t = \int_{0}^{\frac{\pi}{4}} \tan^{-1}\left(\frac{2}{\sqrt{2}(1 + \tan(t))}\right) \mathrm{d}t.
\]

Simplifying:

\[
I = \int_{0}^{\frac{\pi}{4}} \tan^{-1}\left(\frac{\sqrt{2}}{1 + \tan(t)}\right) \mathrm{d}t.
\]

Now, let’s add the original integral \( I \) and this transformed integral:

\[
2I = \int_{0}^{\frac{\pi}{4}} \left[ \tan^{-1}\left(\frac{1 + \tan(t)}{\sqrt{2}}\right) + \tan^{-1}\left(\frac{\sqrt{2}}{1 + \tan(t)}\right) \right] \mathrm{d}t.
\]

Using the identity \( \tan^{-1}(a) + \tan^{-1}\left(\frac{1}{a}\right) = \frac{\pi}{2} \) for \( a > 0 \), we have:

\[
\tan^{-1}\left(\frac{1 + \tan(t)}{\sqrt{2}}\right) + \tan^{-1}\left(\frac{\sqrt{2}}{1 + \tan(t)}\right) = \frac{\pi}{2}.
\]

Thus:

\[
2I = \int_{0}^{\frac{\pi}{4}} \frac{\pi}{2} \mathrm{d}t = \frac{\pi}{2} \cdot \frac{\pi}{4} = \frac{\pi^2}{8}.
\]

Therefore:

\[
I = \frac{\pi^2}{16}.
\]

### Numerical Approximation
The numerical value of \( \frac{\pi^2}{16} \) is approximately:

\[
\frac{\pi^2}{16} \approx 0.6168502751.
\]

### Final Answer
```json
{"answer": "\\frac{\\pi^2}{16}", "numerical_answer": "0.6168502751"}
```