


To solve the definite integral \(\int\limits_0^2 x^{1/2}(2-x)^{-1/2}\cosh\left(\sqrt{x(2-x)}\right)dx\), we proceed with the following steps:

### Step 1: Substitution
First, simplify the argument of the hyperbolic cosine. Note that \(x(2-x) = 1 - (x-1)^2\) (by completing the square). Let \(x = 1 + \sin\theta\), so \(dx = \cos\theta d\theta\). The limits of integration change as follows: when \(x=0\), \(\theta = -\pi/2\); when \(x=2\), \(\theta = \pi/2\).

### Step 2: Simplify the Integrand
Substituting \(x = 1 + \sin\theta\) into the integrand:
- \(x^{1/2} = (1 + \sin\theta)^{1/2}\)
- \((2 - x)^{-1/2} = (1 - \sin\theta)^{-1/2}\)
- \(\sqrt{x(2-x)} = \sqrt{1 - \sin^2\theta} = \cos\theta\)

The product \(x^{1/2}(2 - x)^{-1/2}\) simplifies to \(\sqrt{\frac{1 + \sin\theta}{1 - \sin\theta}} = \frac{1 + \sin\theta}{\cos\theta}\) (since \(\cos\theta > 0\) for \(\theta \in (-\pi/2, \pi/2)\)).

Thus, the integrand becomes:
\[
\frac{1 + \sin\theta}{\cos\theta} \cdot \cosh(\cos\theta) \cdot \cos\theta \, d\theta = (1 + \sin\theta)\cosh(\cos\theta) \, d\theta
\]

### Step 3: Split the Integral
The integral splits into two parts:
\[
\int_{-\pi/2}^{\pi/2} (1 + \sin\theta)\cosh(\cos\theta) \, d\theta = \int_{-\pi/2}^{\pi/2} \cosh(\cos\theta) \, d\theta + \int_{-\pi/2}^{\pi/2} \sin\theta \cosh(\cos\theta) \, d\theta
\]

The second integral vanishes because \(\sin\theta \cosh(\cos\theta)\) is an odd function over symmetric limits. Thus, we only need to evaluate the first integral.

### Step 4: Evaluate the Remaining Integral
The integrand \(\cosh(\cos\theta)\) is even, so:
\[
\int_{-\pi/2}^{\pi/2} \cosh(\cos\theta) \, d\theta = 2 \int_{0}^{\pi/2} \cosh(\cos\theta) \, d\theta
\]

Using the identity \(\cosh(z) = \frac{e^z + e^{-z}}{2}\), we rewrite the integral as:
\[
2 \int_{0}^{\pi/2} \frac{e^{\cos\theta} + e^{-cos\theta}}{2} \, d\theta = \int_{0}^{\pi/2} \left(e^{\cos\theta} + e^{-cos\theta}\right) d\theta
\]

### Step 5: Relate to Modified Bessel Functions
The integral \(\int_{0}^{\pi} e^{z \cos\theta} d\theta = \pi I_0(z)\), where \(I_0(z)\) is the modified Bessel function of the first kind of order 0. For \(z=1\), splitting the integral over \([0, \pi]\) into \([0, \pi/2]\) and \([\pi/2, \pi]\) (with \(\theta \to \pi - \theta\) in the second interval) shows:
\[
\int_{0}^{\pi} e^{\cos\theta} d\theta = \int_{0}^{\pi/2} e^{\cos\theta} d\theta + \int_{0}^{\pi/2} e^{-cos\theta} d\theta
\]

Thus, the original integral simplifies to \(\pi I_0(1)\).

### Numerical Approximation
The modified Bessel function \(I_0(1) \approx 1.26606587775\). Multiplying by \(\pi\) gives:
\[
\pi I_0(1) \approx 3.14159265359 \times 1.26606587775 \approx 3.977463028
\]

### Final Answer
The exact answer is \(\pi I_0(1)\), and the numerical approximation is approximately \(3.9774630280\).

{"answer": "\(\pi I_0(1)\)", "numerical_answer": "3.9774630280"}