<think>
Okay, let's tackle this integral step by step. The integral given is ∫₀¹ x^(-1/4) (1 - x)^(1/4) [1 - √(x(1 - x))]^(-2) dx. Hmm, that looks a bit complicated, but maybe there's a substitution that can simplify it.

First, I notice the terms x and (1 - x) raised to fractional powers. That reminds me of Beta functions or maybe the Beta distribution, which often involve integrals of x^a(1 - x)^b from 0 to 1. But here, there's an additional term [1 - √(x(1 - x))]^(-2), which complicates things. Maybe a substitution can help incorporate that term.

Let me consider a substitution to simplify the expression inside the brackets. Let's set t = √(x(1 - x)). Then, t² = x - x². But I'm not sure if that helps directly. Alternatively, maybe a trigonometric substitution? Since x(1 - x) is similar to sin²θ cos²θ when x = sin²θ. Let's try that.

Let x = sin²θ. Then dx = 2 sinθ cosθ dθ. Let's see what the integral becomes. When x goes from 0 to 1, θ goes from 0 to π/2. Substitute into the integral:

x^(-1/4) becomes (sin²θ)^(-1/4) = sin^(-1/2)θ

(1 - x)^(1/4) becomes (cos²θ)^(1/4) = cos^(1/2)θ

The denominator [1 - √(x(1 - x))]^2 becomes [1 - √(sin²θ cos²θ)]^2 = [1 - sinθ cosθ]^2

So putting it all together, the integral becomes:

∫₀^(π/2) [sin^(-1/2)θ * cos^(1/2)θ] * [1 - sinθ cosθ]^(-2) * 2 sinθ cosθ dθ

Simplify the terms:

sin^(-1/2)θ * cos^(1/2)θ * 2 sinθ cosθ = 2 sin^(1/2)θ * cos^(3/2)θ

So the integral is 2 ∫₀^(π/2) [sin^(1/2)θ cos^(3/2)θ] / [1 - sinθ cosθ]^2 dθ

Hmm, not sure if that's better. Maybe another substitution. Let's see, 1 - sinθ cosθ. Maybe express sinθ cosθ as (1/2) sin2θ. Then 1 - (1/2) sin2θ. But I don't know if that helps.

Alternatively, let's consider another substitution. Let me think about the original integrand again: x^(-1/4)(1 - x)^(1/4)[1 - √(x(1 - x))]^(-2}. Maybe a substitution that combines x and 1 - x. Let's set t = x/(1 - x). Then x = t/(1 + t), 1 - x = 1/(1 + t), dx = dt/(1 + t)^2. Let's try that.

But when x approaches 0, t approaches 0, and x approaches 1, t approaches infinity. The limits become 0 to ∞. Let's substitute:

x^(-1/4) = (t/(1 + t))^(-1/4) = t^(-1/4)(1 + t)^(1/4)

(1 - x)^(1/4) = (1/(1 + t))^(1/4) = (1 + t)^(-1/4)

The denominator [1 - √(x(1 - x))]^2 becomes [1 - √(t/(1 + t) * 1/(1 + t))]^2 = [1 - √(t)/(1 + t)]^2

So the integrand becomes:

t^(-1/4)(1 + t)^(1/4) * (1 + t)^(-1/4) * [1 - √t/(1 + t)]^(-2) * dt/(1 + t)^2

Simplify the terms:

t^(-1/4) * [1 + t]^(1/4 -1/4) = t^(-1/4)

Denominator: [1 - √t/(1 + t)]^2 and the (1 + t)^2 from dx.

So overall, the integrand is t^(-1/4) / [ (1 + t)^2 (1 - √t/(1 + t))^2 ] dt

Hmm, this seems complicated. Let's simplify the denominator:

1 - √t/(1 + t) = [ (1 + t) - √t ] / (1 + t )

So the denominator becomes [ (1 + t - √t ) / (1 + t) ]^2 * (1 + t)^2 = (1 + t - √t )^2

Therefore, the integrand simplifies to t^(-1/4) / (1 + t - √t )^2 dt

Not sure if that's helpful. Maybe another substitution. Let me set u = √t, so t = u², dt = 2u du. Then the integral becomes:

(u²)^(-1/4) * 2u du / (1 + u² - u )^2

Simplify:

u^(-1/2) * 2u du / (1 + u² - u )^2 = 2 u^(1/2) du / (1 + u² - u )^2

Hmm, 1 + u² - u is a quadratic. Let's write it as u² - u +1. The denominator is (u² - u +1)^2. So the integral is 2 ∫ u^(1/2) / (u² - u +1)^2 du from u=0 to u=∞.

This still looks challenging. Maybe another substitution. Let's complete the square in the denominator:

u² - u +1 = (u - 1/2)^2 + 3/4. That might not directly help, but perhaps a substitution. Alternatively, consider rational functions or partial fractions, but with the square in the denominator, that's tough.

Alternatively, maybe a substitution using hypergeometric functions? The integrand has terms u^(1/2) over a quadratic squared. Maybe express in terms of hypergeometric functions, but I'm not sure.

Alternatively, think about integral representations of Beta or Gamma functions. Let me recall that Beta function is ∫₀¹ t^{c-1}(1 - t)^{d - c -1} dt, but not sure.

Wait, maybe using substitution related to the roots of the denominator. Let me factor the denominator. The denominator is (u² - u +1)^2. The roots of u² - u +1 are complex, so maybe not helpful.

Alternatively, consider substitution v = u - 1/2, which centers the quadratic. Let v = u - 1/2, so u = v + 1/2, du = dv. Then the denominator becomes ( (v + 1/2)^2 - (v + 1/2) +1 )^2. Let's compute that:

(v² + v + 1/4) - v -1/2 +1 = v² + v + 1/4 - v -1/2 +1 = v² + (v - v) + (1/4 -1/2 +1) = v² + 3/4. So denominator becomes (v² + 3/4)^2.

The numerator is 2 (v + 1/2)^(1/2). So the integral becomes 2 ∫ (v + 1/2)^(1/2) / (v² + 3/4)^2 dv, from v = -1/2 to v = ∞.

But integrating from v = -1/2 to ∞. Hmm, this might not be easier, but perhaps express in terms of v. Let me check the substitution leads to:

Integral becomes 2 ∫_{-1/2}^∞ (v + 1/2)^(1/2) / (v² + 3/4)^2 dv. Not sure. Maybe split the integral into two parts: from -1/2 to 0 and 0 to ∞. But not sure.

Alternatively, maybe use substitution t = v + 1/2, but that brings us back to u substitution. Hmm.

Alternatively, consider integrating from u=0 to ∞. Let me check the original substitution: when x goes from 0 to1, t = x/(1 -x) goes from 0 to ∞, so u = sqrt(t) goes from 0 to ∞. So the integral after substitution is 2 ∫₀}^∞ u^(1/2) / (u² - u +1)^2 du. Maybe use substitution related to u = tanθ? Let's try u = tanθ, where θ from 0 to π/2. Then du = sec²θ dθ. Let's see:

Denominator becomes (tan²θ - tanθ +1)^2. Hmm, not sure. Alternatively, maybe use substitution u = (sqrt(3)/2) tanθ + 1/2, to make the denominator (v² + 3/4)^2 as before. Let me try that.

Let v = u - 1/2, so denominator is (v² + 3/4)^2. Let v = (sqrt(3)/2) tanφ, so dv = (sqrt(3)/2) sec²φ dφ. Then the integral becomes:

2 ∫ (v + 1/2)^(1/2) / (v² + 3/4)^2 * (sqrt(3)/2) sec²φ dφ. But this seems complicated. The term (v + 1/2)^(1/2) becomes ( (sqrt(3)/2 tanφ) + 1/2 + 1/2 )^(1/2) = (sqrt(3)/2 tanφ + 1 )^(1/2). Not sure.

Alternatively, maybe use substitution z = u² - u +1. Then dz = (2u -1) du. But not sure.

Alternatively, consider integrating by parts. Let me see. Let’s set the integrand as u^(1/2) / (u² - u +1)^2. Let’s see, maybe set w = u^(1/2), dw = (1/2) u^(-1/2) du. But not sure.

Alternatively, look up integral tables. Maybe this integral is a standard form. Let me recall that integrals of the form ∫ x^m (a + b x^n)^p dx can sometimes be expressed in terms of hypergeometric functions. Alternatively, check Gradshteyn and Ryzhik, but since I can't do that, maybe think of expanding the denominator as a series.

The denominator is [1 - √(x(1 - x))]^2. Let me expand this as a binomial series. Since [1 - y]^(-2) = Σ_{k=0}^∞ (k +1) y^k for |y| <1. Here, y = √(x(1 - x)). Since x is between 0 and1, x(1 -x) ≤ 1/4, so y ≤ 1/2, so the series converges.

Therefore, the integral becomes ∫₀¹ x^(-1/4) (1 -x)^(1/4) Σ_{k=0}^∞ (k +1) [x(1 -x)]^{k/2} dx

= Σ_{k=0}^∞ (k +1) ∫₀¹ x^{-1/4 + k/2} (1 -x)^{1/4 + k/2} dx

This is a Beta function! The integral is B(-1/4 + k/2 +1, 1/4 + k/2 +1) = B(3/4 + k/2, 5/4 + k/2)

Recall that B(a,b) = Γ(a)Γ(b)/Γ(a + b). So each term is Γ(3/4 +k/2)Γ(5/4 +k/2)/Γ(2 +k)

But Γ(2 +k) = (k +1)! So the term becomes (k +1) * Γ(3/4 +k/2)Γ(5/4 +k/2)/ (k +1)! ) = Γ(3/4 +k/2)Γ(5/4 +k/2)/k!

But this seems complicated. Let's see if we can express this in terms of known functions. Also, note that Γ(3/4 +k/2)Γ(5/4 +k/2) can be related to Γ functions with duplication formula.

Using the duplication formula: Γ(z)Γ(z +1/2) = 2^{1 - 2z} √π Γ(2z). Let’s set z = 3/4 +k/2. Then Γ(3/4 +k/2)Γ(5/4 +k/2) = Γ(z)Γ(z +1/2) = 2^{1 - 2z} √π Γ(2z)

So substituting z = 3/4 +k/2:

= 2^{1 - 2*(3/4 +k/2)} √π Γ(2*(3/4 +k/2)) = 2^{1 - 3/2 -k} √π Γ(3/2 +k)

Simplify exponent: 1 -3/2 = -1/2, so 2^{-1/2 -k} √π Γ(3/2 +k)

Thus, Γ(3/4 +k/2)Γ(5/4 +k/2) = 2^{-1/2 -k} √π Γ(3/2 +k)

Therefore, each term in the series becomes:

2^{-1/2 -k} √π Γ(3/2 +k) /k! )

So the sum is Σ_{k=0}^∞ (k +1) * [2^{-1/2 -k} √π Γ(3/2 +k) /k! ]

But Γ(3/2 +k) = (1/2 +k)! = (k +1/2)(k -1/2)...(1/2)√π. Wait, Γ(3/2 +k) = (k +1/2)Γ(k +1/2). And Γ(k +1/2) = (2k)! √π / (4^k k! )

Wait, let's recall that Γ(n +1/2) = (2n)! √π / (4^n n! ). So Γ(3/2 +k) = Γ( (k +1) +1/2 ) = (2(k +1))! √π / (4^{k +1} (k +1)! )

Wait, no. Let me check for n =k +1/2. Γ(k +1 +1/2) = (2k +1)! √π / (4^{k +1} (k +1)! )? Wait, no. The formula is Γ(n +1/2) = (2n)! √π / (4^n n! ). So for n =k +1/2, that's not an integer. Wait, maybe I need to adjust.

Actually, the formula is for integer n. For example, Γ(n +1/2) = (2n)! √π / (4^n n! ). So if we set n =k, then Γ(k +1/2) = (2k)! √π / (4^k k! )

But here we have Γ(3/2 +k) = Γ( (k +1) +1/2 ) = Γ( (k +1/2) +1 ) = (k +1/2)Γ(k +1/2 )

So Γ(3/2 +k) = (k +1/2) * Γ(k +1/2 ) = (k +1/2) * (2k)! √π / (4^k k! )

Therefore, substituting back into the term:

Γ(3/2 +k) = (k +1/2) * (2k)! √π / (4^k k! )

So the term becomes:

2^{-1/2 -k} √π * [ (k +1/2) (2k)! √π / (4^k k! ) ] /k! )

Simplify:

2^{-1/2 -k} * π * (k +1/2) (2k)! / (4^k (k! )^2 )

Simplify 4^k = 2^{2k}, so 2^{-1/2 -k} /4^k = 2^{-1/2 -k -2k} = 2^{-1/2 -3k}

Thus, term is π * (k +1/2) (2k)! / (2^{1/2 +3k} (k! )^2 )

So the sum is Σ_{k=0}^∞ π (k +1/2) (2k)! / (2^{1/2 +3k} (k! )^2 )

Hmm, this seems complicated. Let's see if we can relate this to a known series. Let's write (2k)! / (k! )^2 = C(2k, k), the central binomial coefficient. So the term becomes π (k +1/2) C(2k, k) / 2^{1/2 +3k}

So the sum is π / 2^{1/2} Σ_{k=0}^∞ (k +1/2) C(2k, k) / 8^k

Because 2^{3k} =8^k. So π / sqrt(2) Σ_{k=0}^\infty (k +1/2) C(2k,k) (1/8)^k

Now, recall that generating functions for central binomial coefficients. The generating function Σ_{k=0}^\infty C(2k,k) x^k = 1/√(1 -4x). Similarly, Σ_{k=0}^\infty k C(2k,k) x^k = 2x/(1 -4x)^(3/2). Let's check:

Let’s recall that Σ_{k=0}^\infty C(2k,k) x^k = 1/√(1 -4x). Then, differentiating both sides with respect to x:

Σ_{k=0}^\infty k C(2k,k) x^{k-1} = (d/dx) [1/√(1 -4x)] = (1/2)(1 -4x)^{-3/2} *4 = 2 (1 -4x)^{-3/2}

Multiply by x:

Σ_{k=0}^\infty k C(2k,k) x^{k} = 2x (1 -4x)^{-3/2}

So, Σ_{k=0}^\infty (k +1/2) C(2k,k) x^k = Σ_{k=0}^\infty k C(2k,k) x^k + (1/2) Σ_{k=0}^\infty C(2k,k) x^k = 2x (1 -4x)^{-3/2} + (1/2) (1 -4x)^{-1/2}

Therefore, substituting x =1/8:

Σ_{k=0}^\infty (k +1/2) C(2k,k) (1/8)^k = 2*(1/8)*(1 -4*(1/8))^{-3/2} + (1/2)*(1 -4*(1/8))^{-1/2}

Compute 4*(1/8) =1/2, so 1 -1/2 =1/2.

Thus:

= 2*(1/8)*(1/2)^{-3/2} + (1/2)*(1/2)^{-1/2}

Compute (1/2)^{-3/2} =2^{3/2}= 2*sqrt(2), and (1/2)^{-1/2}=sqrt(2)

So:

= 2*(1/8)*2*sqrt(2) + (1/2)*sqrt(2) = (2*1/8*2*sqrt(2)) + (sqrt(2)/2)

Simplify:

First term: (4/8)sqrt(2) = (1/2)sqrt(2)

Second term: (1/2)sqrt(2)

Total: (1/2 +1/2)sqrt(2) = sqrt(2)

Therefore, the sum Σ_{k=0}^\infty (k +1/2) C(2k,k) (1/8)^k = sqrt(2)

Therefore, the original sum is π / sqrt(2) * sqrt(2) = π

So the integral equals π.

Wait, that's surprising! So after all that, the integral simplifies to π. Let me verify this.

Wait, the steps:

1. Expanded the denominator as a binomial series, leading to a sum over k.

2. Each term in the sum was a Beta function, which was expressed in terms of Gamma functions.

3. Using duplication formula and properties of Gamma functions, transformed the terms into a series involving central binomial coefficients.

4. Recognized the series as a known generating function, evaluated it at x=1/8, and found the sum equals sqrt(2).

5. Multiplied by the constants outside the sum (π / sqrt(2)) and got π.

Therefore, the exact value of the integral is π.

For the numerical approximation, π is approximately 3.1415926536. Rounded to 10 decimal places, that's 3.1415926536.

But wait, let me check with a numerical approximation of the integral to confirm. Let's compute the integral numerically to see if it's indeed π.

Alternatively, since the integral is π, the numerical value should be approximately 3.1415926536. Let me verify with a quick estimation.

Suppose we take x=0.5, the integrand becomes (0.5)^(-1/4)*(0.5)^(1/4)*[1 - sqrt(0.5*0.5)]^{-2} = (0.5)^{(-1/4 +1/4)} * [1 - 0.5]^{-2} = 1 * (0.5)^{-2} =4. But the integral over 0 to1 would have contributions from all points. But given the steps above, the analytical result is π, so numerical approximation should match.

Therefore, the exact answer is π, and the numerical approximation is approximately 3.1415926536.
</think>

{"answer": "\\pi", "numerical_answer": "3.1415926536"}