Let's denote the integral as
\[
I = \int_0^1 x \sin(x) \ln \left( \frac{1 + \sqrt{1 - x^2}}{1 - \sqrt{1 - x^2}} \right) dx
\]
where for clarity I have omitted the constant 1.0 as it doesn't affect the variables.

---

### Step 1: Simplify the logarithmic term

Recall:
\[
\ln\left(\frac{1 + y}{1 - y}\right) = 2 \tanh^{-1} y, \quad |y| < 1
\]
If \( y = \sqrt{1-x^2} \):
\[
\ln\left(\frac{1 + \sqrt{1-x^2}}{1 - \sqrt{1-x^2}}\right) = 2 \tanh^{-1}\left( \sqrt{1-x^2} \right)
\]

Thus,
\[
I = 2 \int_0^1 x \sin x \tanh^{-1} \left( \sqrt{1-x^2} \right) dx
\]

---

### Step 2: Substitution to further simplify

Let’s let \( x = \sin\theta \), for \( \theta \in [0, \frac{\pi}{2}] \):

- \( dx = \cos\theta d\theta \)
- \( x = \sin\theta \)
- \( \sqrt{1-x^2} = \cos\theta \)

Thus,
\[
I = 2 \int_{\theta=0}^{\theta=\pi/2} \sin\theta \sin(\sin\theta) \tanh^{-1}(\cos\theta) \cos\theta d\theta
\]

---

### Step 3: Series expansion OR alternate method

Instead, use the following result:
\[
\tanh^{-1} y = \frac{1}{2} \ln \left( \frac{1+y}{1-y} \right), \quad y = \sqrt{1-x^2}
\]
But recall that (from tables/integrals involving inverse hyperbolic tangent and substitutions in definite integrals):

Alternatively, let's attempt to express the integral as a series, or find a more direct exact expression.

Rewriting:
\[
\tanh^{-1}(\sqrt{1-x^2}) = \sum_{n=0}^{\infty} \frac{(\sqrt{1-x^2})^{2n+1}}{2n+1}
\]
But \((\sqrt{1-x^2})^{2n+1} = (1-x^2)^{n+\frac{1}{2}}\), but then the integration gets subtle.

---

### Step 4: Alternate substitution

Recall:
\[
\ln\left( \frac{1+\sqrt{1-x^2}}{1-\sqrt{1-x^2}} \right) = 2 \arcsin x
\]

**Proof of identity:** If \( x = \sin\theta \), then \( \sqrt{1-x^2} = \cos\theta \), and
\[
\frac{1+\cos\theta}{1-\cos\theta} = \frac{2\cos^2(\theta/2)}{2\sin^2(\theta/2)} = \cot^2(\theta/2)
\]
But this gives:
\[
\ln\left( \frac{1+\cos\theta}{1-\cos\theta} \right) = 2\ln \cot(\theta/2)
\]
But with \( \sin\theta \) rather than \( \cos\theta \), this is subtle.

Actually,
\[
\arcsin x = \arctan\left( \frac{x}{\sqrt{1-x^2}} \right)
\]
But per standard identities:
\[
\ln\left( \frac{1+\sqrt{1-x^2}}{1-\sqrt{1-x^2}} \right) = 2 \arccosh \left( \frac{1}{x} \right), \quad x \in (0,1)
\]
But for \( x\in[0,1] \), \( \arccosh\left( \frac{1}{x} \right) \) is real.

But for \( x \in [0,1] \):
\[
\ln\left( \frac{1+\sqrt{1-x^2}}{1-\sqrt{1-x^2}} \right) = 2 \arcsin x
\]
**[This is in fact a correct identity.]**

#### Let's check:

Let \( x = \sin \theta \), \( \theta \in [0, \frac{\pi}{2}] \).

- \( \sqrt{1-x^2} = \cos \theta \)

Now,
\[
\ln\left( \frac{1+\cos\theta}{1-\cos\theta} \right) = \ln \left( \frac{2\cos^2(\theta/2)}{2\sin^2(\theta/2)} \right) = 2\ln \cot(\theta/2)
\]
But for \( \sqrt{1-x^2} \):
\[
\ln\left( \frac{1+\sqrt{1-x^2}}{1-\sqrt{1-x^2}} \right) = \ln \left( \frac{1+\cos\theta}{1-\cos\theta} \right) = 2\ln \cot(\theta/2)
\]
But this is not \( 2\arcsin x \), so it is not straightforward.

Alternatively, let's use the series expansion for \( \tanh^{-1} \):

\[
\tanh^{-1}(y) = \sum_{k=0}^\infty \frac{y^{2k+1}}{2k+1} \,\,\,\, |y| < 1
\]
So,
\[
\tanh^{-1}\left( \sqrt{1-x^2} \right) = \sum_{k=0}^\infty \frac{ (1-x^2)^{k+\frac{1}{2}} }{2k+1 }
\]
But, with the factor \( x\sin x \), integrating term by term is difficult.

---

### Step 5: Attempt to express as a single definite integral

Let's make an alternative substitution:

Let’s use integration by parts.

Set:

- \( u = \ln\left( \frac{1+\sqrt{1-x^2}}{1-\sqrt{1-x^2}} \right) \)
- \( dv = x \sin x dx \)

First, compute \( \int x \sin x dx \):

Let’s recall:
\[
\int x \sin x dx = -x \cos x + \int \cos x dx = -x \cos x + \sin x + C
\]

Set:
- \( u = \ln\left( \frac{1+\sqrt{1-x^2}}{1-\sqrt{1-x^2}} \right) \)
- \( dv = x \sin x dx \implies v = -x \cos x + \sin x \)

Thus,
\[
I = u v \Big|_0^1 - \int_0^1 v \, du
\]
Now, we need to compute \( du \).

---

#### Compute \( du \):

Let \( f(x) = \ln\left( \frac{1+\sqrt{1-x^2}}{1-\sqrt{1-x^2}} \right) \)

Let’s differentiate:

\[
\frac{d}{dx}\left( \ln \left( \frac{1+\sqrt{1-x^2}}{1-\sqrt{1-x^2}} \right) \right) = \frac{d}{dx} \left( \ln(1+\sqrt{1-x^2}) - \ln(1-\sqrt{1-x^2}) \right )
\]
\[
= \frac{1}{1+\sqrt{1-x^2}} \cdot \frac{-x}{\sqrt{1-x^2}} - \frac{1}{1-\sqrt{1-x^2}} \cdot \frac{-x}{\sqrt{1-x^2}}
\]
\[
= \frac{-x}{\sqrt{1-x^2}} \left( \frac{1}{1+\sqrt{1-x^2}} - \frac{1}{1-\sqrt{1-x^2}} \right )
\]

Compute the parenthesis:

\[
\frac{1}{1+\sqrt{1-x^2}} - \frac{1}{1-\sqrt{1-x^2}} = \frac{1-\sqrt{1-x^2} - 1 - \sqrt{1-x^2}}{1 - (1-x^2)}
= \frac{-2\sqrt{1-x^2}}{x^2}
\]

Thus,
\[
\frac{d}{dx} f(x)
= \frac{-x}{\sqrt{1-x^2}} \cdot \left( \frac{-2\sqrt{1-x^2}}{x^2} \right )
= \frac{2x}{x^2}
= \frac{2}{x}
\]
So the derivative is extremely simple:
\[
du = f'(x) dx = \frac{2}{x} dx
\]
---

### Step 6: Plug into Integration by Parts

Recall:
\[
I = u v |_{x=0}^{x=1} - \int_{x=0}^{x=1} v \cdot du
\]
\[
I = \left[ \ln\left( \frac{1+\sqrt{1-x^2}}{1-\sqrt{1-x^2}} \right ) \cdot (-x \cos x + \sin x) \right ]_{0}^{1} - \int_{0}^{1} (-x \cos x + \sin x ) \cdot \frac{2}{x} dx
\]
\[
= \left[ \ln\left( \frac{1+\sqrt{1-x^2}}{1-\sqrt{1-x^2}} \right ) \cdot (-x \cos x + \sin x) \right ]_{0}^{1} - 2 \int_{0}^{1} \left( -\cos x + \frac{\sin x}{x} \right ) dx
\]

---

### Step 7: Evaluate Boundary Terms

First, at \( x = 1 \):

- \( \sqrt{1-x^2} = 0 \)
- \( \ln\left( \frac{1+0}{1-0} \right ) = \ln(1) = 0 \)

So, term at \( x=1 \) is zero.

At \( x=0 \):

- \( \sqrt{1-0^2} = 1 \)
- \( \ln\left( \frac{1+1}{1-1} \right ) = \ln\left( \frac{2}{0} \right ) \rightarrow +\infty \)
- But let's check what happens to \( -x \cos x + \sin x \) as \( x\to 0 \): \( -0 \cdot 1 + 0 = 0 \)

So, the boundary term at \( x=0 \) is \( 0 \). (To confirm: both \( u \to \infty \), \( v \to 0 \), but their product tends to zero.)

Let’s check the limit carefully:
\[
\lim_{x \to 0^+} \ln\left( \frac{1+\sqrt{1-x^2}}{1-\sqrt{1-x^2}} \right ) \cdot ( -x \cos x + \sin x ) = \lim_{x \to 0^+} (2 \arcsin x) (-x \cos x + \sin x)
\]
But as \( x \to 0 \), \( \arcsin x \sim x \) and \( -x \cos x + \sin x \sim -x + x = 0 \).
So, the term at \( x=0 \) is 0.

Thus, the only contribution is from the integral:

\[
I = -2 \int_0^1 \left( -\cos x + \frac{\sin x}{x} \right ) dx
\]
\[
= 2 \int_0^1 \cos x dx - 2 \int_0^1 \frac{\sin x}{x} dx
\]

Evaluate the first integral:
\[
\int_0^1 \cos x dx = \sin 1 - \sin 0 = \sin 1
\]

The second integral is the sine integral:
\[
\int_0^1 \frac{\sin x}{x} dx = \operatorname{Si}(1)
\]

So:

\[
I = 2 \sin 1 - 2 \operatorname{Si}(1)
\]

where \( \operatorname{Si}(x) = \int_0^x \frac{\sin t}{t} dt \) is the sine integral function.

---

### Step 8: Final exact answer

So our exact answer is:
\[
I = 2 \sin 1 - 2\,\operatorname{Si}(1)
\]


### Step 9: Numerical approximation
Let’s compute this value to 10 decimal places.

- \( \sin 1 \approx 0.8414709848 \)
- \( \operatorname{Si}(1) \approx 0.9460830704 \)

Thus,
\[
I \approx 2 \times 0.8414709848 - 2 \times 0.9460830704 = 1.6829419696 - 1.8921661408 = -0.2092241712
\]

---

### Step 10: JSON output

```json
{"answer": "2\\sin 1 - 2\\operatorname{Si}(1)", "numerical_answer": "-0.2092241712"}
```