To solve the definite integral \(\int_{0}^{1} \left( \frac{1}{x} - \left\lfloor \frac{1}{x} \right\rfloor \right) \, dx\), we need to carefully analyze the integrand \(\frac{1}{x} - \left\lfloor \frac{1}{x} \right\rfloor\).

### Step 1: Analyze the Integrand

The floor function \(\left\lfloor \frac{1}{x} \right\rfloor\) represents the greatest integer less than or equal to \(\frac{1}{x}\). For \(x\) in the interval \((0, 1]\), \(\frac{1}{x}\) ranges from \([1, \infty)\).

### Step 2: Break the Integral into Parts

We can break the integral into parts where \(\left\lfloor \frac{1}{x} \right\rfloor\) is constant. For each integer \(n \geq 1\), consider the interval where \(\left\lfloor \frac{1}{x} \right\rfloor = n\). This happens when \(n \leq \frac{1}{x} < n+1\), or equivalently, \(\frac{1}{n+1} < x \leq \frac{1}{n}\).

Thus, the integral can be written as:
\[
\int_{0}^{1} \left( \frac{1}{x} - \left\lfloor \frac{1}{x} \right\rfloor \right) \, dx = \sum_{n=1}^{\infty} \int_{\frac{1}{n+1}}^{\frac{1}{n}} \left( \frac{1}{x} - n \right) \, dx
\]

### Step 3: Evaluate Each Integral

For each \(n\), we evaluate the integral:
\[
\int_{\frac{1}{n+1}}^{\frac{1}{n}} \left( \frac{1}{x} - n \right) \, dx
\]

First, compute the integral of \(\frac{1}{x}\):
\[
\int_{\frac{1}{n+1}}^{\frac{1}{n}} \frac{1}{x} \, dx = \ln x \Big|_{\frac{1}{n+1}}^{\frac{1}{n}} = \ln \left( \frac{1}{n} \right) - \ln \left( \frac{1}{n+1} \right) = \ln \left( \frac{n+1}{n} \right) = \ln \left( 1 + \frac{1}{n} \right)
\]

Next, compute the integral of \(n\):
\[
\int_{\frac{1}{n+1}}^{\frac{1}{n}} n \, dx = n \left( \frac{1}{n} - \frac{1}{n+1} \right) = n \left( \frac{1}{n(n+1)} \right) = \frac{1}{n+1}
\]

Combining these results, we get:
\[
\int_{\frac{1}{n+1}}^{\frac{1}{n}} \left( \frac{1}{x} - n \right) \, dx = \ln \left( 1 + \frac{1}{n} \right) - \frac{1}{n+1}
\]

### Step 4: Sum the Series

The integral is then:
\[
\sum_{n=1}^{\infty} \left( \ln \left( 1 + \frac{1}{n} \right) - \frac{1}{n+1} \right)
\]

This series can be simplified using the properties of logarithms and known series results. The series \(\sum_{n=1}^{\infty} \ln \left( 1 + \frac{1}{n} \right)\) is known to converge to \(\ln \left( \prod_{n=1}^{\infty} \left( 1 + \frac{1}{n} \right) \right)\), which is \(\ln \left( \lim_{n \to \infty} \frac{n+1}{n} \right) = \ln e = 1\).

The series \(\sum_{n=1}^{\infty} \frac{1}{n+1}\) is the harmonic series shifted by one, which diverges. However, the difference between these series converges to a known constant, the Euler-Mascheroni constant \(\gamma\).

Thus, the integral evaluates to:
\[
\sum_{n=1}^{\infty} \left( \ln \left( 1 + \frac{1}{n} \right) - \frac{1}{n+1} \right) = 1 - \gamma
\]

### Step 5: Numerical Approximation

The Euler-Mascheroni constant \(\gamma\) is approximately 0.5772156649. Therefore, the numerical approximation of the result is:
\[
1 - \gamma \approx 1 - 0.5772156649 = 0.4227843351
\]

### Final Answer

\[
\boxed{
\begin{aligned}
\text{"answer": "1 - \gamma", "numerical_answer": "0.4227843351"}
\end{aligned}
}
\]