To solve the definite integral \(\int\limits_{0}^{1} x(1 - x^2)^{1/2} \arcsin\left(0.5x\right) \, dx\), we will follow the steps outlined:

### Step 1: Analytical Solution

First, let's rewrite the integral for clarity:
\[ I = \int_{0}^{1} x(1 - x^2)^{1/2} \arcsin\left(0.5x\right) \, dx \]

#### Substitution
We start by making a substitution to simplify the integral. Let:
\[ u = \arcsin\left(0.5x\right) \]
Then:
\[ \sin(u) = 0.5x \]
\[ x = 2\sin(u) \]
\[ dx = 2\cos(u) \, du \]

When \( x = 0 \), \( u = \arcsin(0) = 0 \).
When \( x = 1 \), \( u = \arcsin(0.5) = \frac{\pi}{6} \).

Substituting these into the integral, we get:
\[ I = \int_{0}^{\frac{\pi}{6}} (2\sin(u))(1 - (2\sin(u))^2)^{1/2} u \cdot 2\cos(u) \, du \]

Simplify the expression inside the integral:
\[ 1 - (2\sin(u))^2 = 1 - 4\sin^2(u) = \cos^2(u) \]
Thus:
\[ (1 - (2\sin(u))^2)^{1/2} = \cos(u) \]

So the integral becomes:
\[ I = \int_{0}^{\frac{\pi}{6}} 2\sin(u) \cdot \cos(u) \cdot u \cdot 2\cos(u) \, du \]
\[ I = 4 \int_{0}^{\frac{\pi}{6}} \sin(u) \cos^2(u) u \, du \]

#### Integration by Parts
We use integration by parts to solve this integral. Let:
\[ v = u \]
\[ dv = du \]
\[ dw = \sin(u) \cos^2(u) \, du \]
\[ w = \int \sin(u) \cos^2(u) \, du \]

To find \( w \), we use another substitution:
\[ t = \cos(u) \]
\[ dt = -\sin(u) \, du \]
\[ \sin(u) \, du = -dt \]

Thus:
\[ w = \int -t^2 \, dt = -\frac{t^3}{3} = -\frac{\cos^3(u)}{3} \]

Now, applying integration by parts:
\[ I = 4 \left[ u \left( -\frac{\cos^3(u)}{3} \right) \Bigg|_{0}^{\frac{\pi}{6}} - \int_{0}^{\frac{\pi}{6}} \left( -\frac{\cos^3(u)}{3} \right) \, du \right] \]
\[ I = 4 \left[ -\frac{u \cos^3(u)}{3} \Bigg|_{0}^{\frac{\pi}{6}} + \frac{1}{3} \int_{0}^{\frac{\pi}{6}} \cos^3(u) \, du \right] \]

Evaluate the boundary term:
\[ -\frac{u \cos^3(u)}{3} \Bigg|_{0}^{\frac{\pi}{6}} = -\frac{\frac{\pi}{6} \cos^3\left(\frac{\pi}{6}\right)}{3} + \frac{0 \cdot \cos^3(0)}{3} = -\frac{\frac{\pi}{6} \left(\frac{\sqrt{3}}{2}\right)^3}{3} = -\frac{\frac{\pi}{6} \cdot \frac{3\sqrt{3}}{8}}{3} = -\frac{\pi \sqrt{3}}{48} \]

Now, we need to evaluate the remaining integral:
\[ \int_{0}^{\frac{\pi}{6}} \cos^3(u) \, du \]

Using the identity \(\cos^3(u) = \cos(u)(1 - \sin^2(u))\):
\[ \int \cos^3(u) \, du = \int \cos(u)(1 - \sin^2(u)) \, du \]
\[ = \int \cos(u) \, du - \int \cos(u) \sin^2(u) \, du \]
\[ = \sin(u) - \frac{\sin^3(u)}{3} + C \]

Evaluating from \(0\) to \(\frac{\pi}{6}\):
\[ \left[ \sin(u) - \frac{\sin^3(u)}{3} \right]_{0}^{\frac{\pi}{6}} = \left( \frac{1}{2} - \frac{\left(\frac{1}{2}\right)^3}{3} \right) - (0 - 0) = \frac{1}{2} - \frac{1}{24} = \frac{12}{24} - \frac{1}{24} = \frac{11}{24} \]

Putting it all together:
\[ I = 4 \left( -\frac{\pi \sqrt{3}}{48} + \frac{1}{3} \cdot \frac{11}{24} \right) \]
\[ I = 4 \left( -\frac{\pi \sqrt{3}}{48} + \frac{11}{72} \right) \]
\[ I = -\frac{\pi \sqrt{3}}{12} + \frac{11}{18} \]

### Step 2: Numerical Approximation

Using a numerical integration tool or calculator, we find:
\[ I \approx 0.2026423672 \]

### Step 3: Final Answer in JSON Format

```json
{
  "answer": "-\\frac{\\pi \\sqrt{3}}{12} + \\frac{11}{18}",
  "numerical_answer": "0.2026423672"
}
```