# Evaluating $\int\limits_{0}^{2}H_{3}\left(\sqrt{x(2-x)}\right)dx$

First, I need to identify what $H_3$ represents. $H_3$ is the 3rd Hermite polynomial, which is:

$H_3(x) = 8x^3 - 12x$

So I need to calculate:
$\int\limits_{0}^{2}H_{3}\left(\sqrt{x(2-x)}\right)dx = \int\limits_{0}^{2}[8(\sqrt{x(2-x)})^3 - 12\sqrt{x(2-x)}]dx$

## Step 1: Simplify the integrand
Let's examine $\sqrt{x(2-x)}$ for $x \in [0,2]$.

This can be rewritten as:
$\sqrt{x(2-x)} = \sqrt{2x-x^2} = \sqrt{1-(x-1)^2}$

This shows that $\sqrt{x(2-x)}$ is a semicircle with radius 1 centered at $x=1$.

Let's make the substitution $x = 1 + \sin\theta$, which means $dx = \cos\theta\,d\theta$.

When $x = 0$, we have $1 + \sin\theta = 0$, so $\theta = -\frac{\pi}{2}$.
When $x = 2$, we have $1 + \sin\theta = 2$, so $\theta = \frac{\pi}{2}$.

With this substitution:
$\sqrt{x(2-x)} = \sqrt{1-(x-1)^2} = \sqrt{1-\sin^2\theta} = \cos\theta$

## Step 2: Transform the integral
The integral becomes:
$\int\limits_{-\pi/2}^{\pi/2}[8\cos^3\theta - 12\cos\theta]\cos\theta\,d\theta = \int\limits_{-\pi/2}^{\pi/2}[8\cos^4\theta - 12\cos^2\theta]\,d\theta$

## Step 3: Use standard trigonometric integrals
For $\cos^4\theta$:
$\cos^4\theta = \frac{1}{8}[3 + 4\cos(2\theta) + \cos(4\theta)]$

For $\cos^2\theta$:
$\cos^2\theta = \frac{1}{2}[1 + \cos(2\theta)]$

## Step 4: Substitute and integrate
$\int\limits_{-\pi/2}^{\pi/2}[8\cos^4\theta - 12\cos^2\theta]\,d\theta$
$= \int\limits_{-\pi/2}^{\pi/2}[8(\frac{1}{8}[3 + 4\cos(2\theta) + \cos(4\theta)]) - 12(\frac{1}{2}[1 + \cos(2\theta)])]\,d\theta$
$= \int\limits_{-\pi/2}^{\pi/2}[3 + 4\cos(2\theta) + \cos(4\theta) - 6 - 6\cos(2\theta)]\,d\theta$
$= \int\limits_{-\pi/2}^{\pi/2}[-3 - 2\cos(2\theta) + \cos(4\theta)]\,d\theta$

Now I integrate each term:
$\int -3\,d\theta = -3\theta$
$\int -2\cos(2\theta)\,d\theta = -2\cdot\frac{\sin(2\theta)}{2} = -\sin(2\theta)$
$\int \cos(4\theta)\,d\theta = \frac{\sin(4\theta)}{4}$

Evaluating from $-\pi/2$ to $\pi/2$:
$[-3\theta - \sin(2\theta) + \frac{\sin(4\theta)}{4}]_{-\pi/2}^{\pi/2}$

At $\theta = \pi/2$: $-3\cdot\frac{\pi}{2} - \sin(\pi) + \frac{\sin(2\pi)}{4} = -\frac{3\pi}{2} - 0 + 0 = -\frac{3\pi}{2}$
At $\theta = -\pi/2$: $-3\cdot(-\frac{\pi}{2}) - \sin(-\pi) + \frac{\sin(-2\pi)}{4} = \frac{3\pi}{2} - 0 + 0 = \frac{3\pi}{2}$

The result is: $-\frac{3\pi}{2} - \frac{3\pi}{2} = -3\pi$

## Numerical approximation
$-3\pi \approx -9.4247779607693797153879301498385$

Rounded to 10 decimal places: $-9.4247779608$

{"answer": "-3\\pi", "numerical_answer": "-9.4247779608"}