# Evaluating $\int_{\pi/6}^{\pi/3}\frac{\sin(x)+\cos(x)}{\sqrt{\sin(2x)}}\text{ d}x$

## Step 1: Simplify the integrand
Let's first recall that $\sin(2x) = 2\sin(x)\cos(x)$. So:

$$\frac{\sin(x)+\cos(x)}{\sqrt{\sin(2x)}} = \frac{\sin(x)+\cos(x)}{\sqrt{2\sin(x)\cos(x)}} = \frac{\sin(x)+\cos(x)}{\sqrt{2}\sqrt{\sin(x)\cos(x)}}$$

## Step 2: Make a substitution
Let's use the substitution $u = x$, so $du = dx$. This doesn't change the integral, but helps us keep track of the variable:

$$\int_{\pi/6}^{\pi/3}\frac{\sin(x)+\cos(x)}{\sqrt{2\sin(x)\cos(x)}}\text{ d}x = \frac{1}{\sqrt{2}}\int_{\pi/6}^{\pi/3}\frac{\sin(u)+\cos(u)}{\sqrt{\sin(u)\cos(u)}}\text{ d}u$$

## Step 3: Split the integral
We can split this into two integrals:

$$\frac{1}{\sqrt{2}}\int_{\pi/6}^{\pi/3}\frac{\sin(u)}{\sqrt{\sin(u)\cos(u)}}\text{ d}u + \frac{1}{\sqrt{2}}\int_{\pi/6}^{\pi/3}\frac{\cos(u)}{\sqrt{\sin(u)\cos(u)}}\text{ d}u$$

## Step 4: Simplify each integrand
For the first integral:
$$\frac{1}{\sqrt{2}}\int_{\pi/6}^{\pi/3}\frac{\sin(u)}{\sqrt{\sin(u)\cos(u)}}\text{ d}u = \frac{1}{\sqrt{2}}\int_{\pi/6}^{\pi/3}\frac{\sqrt{\sin(u)}}{\sqrt{\cos(u)}}\text{ d}u$$

For the second integral:
$$\frac{1}{\sqrt{2}}\int_{\pi/6}^{\pi/3}\frac{\cos(u)}{\sqrt{\sin(u)\cos(u)}}\text{ d}u = \frac{1}{\sqrt{2}}\int_{\pi/6}^{\pi/3}\frac{\sqrt{\cos(u)}}{\sqrt{\sin(u)}}\text{ d}u$$

## Step 5: Evaluate these integrals
For the first integral, let's use the substitution $v = \sqrt{\tan(u)}$. Then:
- $\tan(u) = v^2$
- $u = \arctan(v^2)$
- $du = \frac{2v}{1+v^4}dv$
- $\sin(u) = \frac{v^2}{\sqrt{1+v^4}}$
- $\cos(u) = \frac{1}{\sqrt{1+v^4}}$

This gives us:
$$\frac{\sqrt{\sin(u)}}{\sqrt{\cos(u)}} = \frac{\sqrt{\frac{v^2}{\sqrt{1+v^4}}}}{\sqrt{\frac{1}{\sqrt{1+v^4}}}} = v$$

So the first integral becomes:
$$\frac{1}{\sqrt{2}}\int_{\pi/6}^{\pi/3}v \cdot \frac{2v}{1+v^4}dv = \frac{1}{\sqrt{2}}\int_{\pi/6}^{\pi/3}\frac{2v^2}{1+v^4}dv$$

Similarly, for the second integral, we can use the substitution $w = \sqrt{\cot(u)}$ to get:
$$\frac{1}{\sqrt{2}}\int_{\pi/6}^{\pi/3}\frac{\sqrt{\cos(u)}}{\sqrt{\sin(u)}}\text{ d}u = \frac{1}{\sqrt{2}}\int_{\pi/6}^{\pi/3}w \cdot \frac{-2w}{1+w^4}dw = -\frac{1}{\sqrt{2}}\int_{\pi/6}^{\pi/3}\frac{2w^2}{1+w^4}dw$$

## Step 6: Combining the results
Looking at these two integrals, we can see they are related. In fact, when we change variables properly and set the appropriate limits, we find:

$$\int_{\pi/6}^{\pi/3}\frac{\sin(x)+\cos(x)}{\sqrt{\sin(2x)}}\text{ d}x = \frac{1}{\sqrt{2}}\int_{\pi/6}^{\pi/3}\frac{\sqrt{\sin(u)}}{\sqrt{\cos(u)}}\text{ d}u + \frac{1}{\sqrt{2}}\int_{\pi/6}^{\pi/3}\frac{\sqrt{\cos(u)}}{\sqrt{\sin(u)}}\text{ d}u$$

I'll now use a different approach for clarity.

## Alternative solution
Let's use the substitution $t = \tan(x)$. Then:
- $dx = \frac{dt}{1+t^2}$
- $\sin(x) = \frac{t}{\sqrt{1+t^2}}$
- $\cos(x) = \frac{1}{\sqrt{1+t^2}}$
- $\sin(2x) = \frac{2t}{1+t^2}$

When $x = \pi/6$, $t = \tan(\pi/6) = \frac{1}{\sqrt{3}}$
When $x = \pi/3$, $t = \tan(\pi/3) = \sqrt{3}$

After substitution and simplification, we get:
$$\int_{\pi/6}^{\pi/3}\frac{\sin(x)+\cos(x)}{\sqrt{\sin(2x)}}\text{ d}x = \int_{1/\sqrt{3}}^{\sqrt{3}}\frac{t+1}{\sqrt{1+t^2}\sqrt{\frac{2t}{1+t^2}}}\frac{dt}{1+t^2}$$

Simplifying:
$$= \int_{1/\sqrt{3}}^{\sqrt{3}}\frac{t+1}{\sqrt{2t(1+t^2)}}\frac{dt}{1+t^2} = \frac{1}{\sqrt{2}}\int_{1/\sqrt{3}}^{\sqrt{3}}\frac{t+1}{\sqrt{t}(1+t^2)}dt$$

Let's split this into two integrals:
$$\frac{1}{\sqrt{2}}\int_{1/\sqrt{3}}^{\sqrt{3}}\frac{t}{\sqrt{t}(1+t^2)}dt + \frac{1}{\sqrt{2}}\int_{1/\sqrt{3}}^{\sqrt{3}}\frac{1}{\sqrt{t}(1+t^2)}dt$$

For the first integral:
$$\frac{1}{\sqrt{2}}\int_{1/\sqrt{3}}^{\sqrt{3}}\frac{t}{\sqrt{t}(1+t^2)}dt = \frac{1}{\sqrt{2}}\int_{1/\sqrt{3}}^{\sqrt{3}}\frac{\sqrt{t}}{1+t^2}dt$$

For the second integral:
$$\frac{1}{\sqrt{2}}\int_{1/\sqrt{3}}^{\sqrt{3}}\frac{1}{\sqrt{t}(1+t^2)}dt$$

Using standard integration techniques:
- For the first integral, substitute $u = t^2$ to get $\frac{1}{2\sqrt{2}}\int_{1/3}^{3}\frac{1}{1+u}du = \frac{1}{2\sqrt{2}}[\ln(1+u)]_{1/3}^{3} = \frac{1}{2\sqrt{2}}[\ln(4) - \ln(4/3)] = \frac{1}{2\sqrt{2}}\ln(3)$

- For the second integral, we can use partial fractions and substitution to evaluate it to $\frac{1}{\sqrt{2}}[2\arctan(t)]_{1/\sqrt{3}}^{\sqrt{3}} = \frac{1}{\sqrt{2}}[2\arctan(\sqrt{3}) - 2\arctan(1/\sqrt{3})] = \frac{1}{\sqrt{2}}[2\cdot\frac{\pi}{3} - 2\cdot\frac{\pi}{6}] = \frac{\pi}{2\sqrt{2}}$

Therefore:
$$\int_{\pi/6}^{\pi/3}\frac{\sin(x)+\cos(x)}{\sqrt{\sin(2x)}}\text{ d}x = \frac{1}{2\sqrt{2}}\ln(3) + \frac{\pi}{2\sqrt{2}} = \frac{\ln(3) + \pi}{2\sqrt{2}}$$

## Numerical approximation
$\frac{\ln(3) + \pi}{2\sqrt{2}} \approx \frac{1.0986 + 3.1416}{2\sqrt{2}} \approx \frac{4.2402}{2.8284} \approx 1.4991781753$

Let me calculate this more precisely:
$\ln(3) = 1.0986122887$
$\pi = 3.1415926536$
$2\sqrt{2} = 2.8284271247$
$\frac{\ln(3) + \pi}{2\sqrt{2}} = \frac{4.2402049423}{2.8284271247} = 1.4991781755$

{"answer": "\\frac{\\ln(3) + \\pi}{2\\sqrt{2}}", "numerical_answer": "1.4991781755"}