To evaluate the definite integral

$$
\int_0^1 \frac{\sin(\log x) - \log x}{\log^2 x} \, dx,
$$

we proceed through a sequence of transformations and analytical techniques.

---

### **Step 1: Substitution**

Let us perform the substitution $ t = \log x $, so that $ x = e^t $, and $ dx = e^t \, dt $. The limits of integration transform as follows:

- When $ x = 0 $, $ t \to -\infty $
- When $ x = 1 $, $ t = 0 $

Substituting into the integral:

$$
\int_0^1 \frac{\sin(\log x) - \log x}{\log^2 x} \, dx = \int_{-\infty}^0 \frac{\sin t - t}{t^2} e^t \, dt.
$$

To simplify the domain, we perform another substitution: $ u = -t $, so that $ t = -u $, $ dt = -du $, and the limits become $ u = 0 $ to $ u = \infty $. The integral becomes:

$$
\int_0^\infty \frac{u - \sin u}{u^2} e^{-u} \, du.
$$

---

### **Step 2: Series Expansion**

We expand the numerator $ u - \sin u $ using the Taylor series of $ \sin u $:

$$
\sin u = u - \frac{u^3}{3!} + \frac{u^5}{5!} - \cdots
\Rightarrow u - \sin u = \frac{u^3}{3!} - \frac{u^5}{5!} + \cdots
$$

Thus,

$$
\frac{u - \sin u}{u^2} = \frac{u^3}{6u^2} - \frac{u^5}{120u^2} + \cdots = \frac{u}{6} - \frac{u^3}{120} + \cdots
$$

Multiplying by $ e^{-u} $, we get:

$$
\frac{u - \sin u}{u^2} e^{-u} = \sum_{k=1}^\infty \frac{(-1)^{k+1}}{(2k+1)!} u^{2k-1} e^{-u}.
$$

Now, integrate term-by-term:

$$
\int_0^\infty u^{2k-1} e^{-u} \, du = (2k-1)!
$$

So the integral becomes:

$$
\sum_{k=1}^\infty \frac{(-1)^{k+1}}{(2k+1)!} \cdot (2k-1)! = \sum_{k=1}^\infty \frac{(-1)^{k+1}}{2k(2k+1)}.
$$

This series can be evaluated by splitting the terms:

$$
\sum_{k=1}^\infty \frac{(-1)^{k+1}}{2k(2k+1)} = \sum_{k=1}^\infty \left( \frac{(-1)^{k+1}}{2k} - \frac{(-1)^{k+1}}{2k+1} \right)
$$

This separates into two convergent series:

- $ \sum_{k=1}^\infty \frac{(-1)^{k+1}}{2k} = \frac{1}{2} \sum_{k=1}^\infty \frac{(-1)^{k+1}}{k} = \frac{1}{2} \ln 2 $
- $ \sum_{k=1}^\infty \frac{(-1)^{k+1}}{2k+1} = 1 - \frac{\pi}{4} $

Therefore, the exact value of the integral is:

$$
\frac{\ln 2}{2} - \left(1 - \frac{\pi}{4}\right) = \frac{\pi}{4} + \frac{\ln 2}{2} - 1
$$

---

### **Step 3: Numerical Approximation**

Using known values:

- $ \frac{\pi}{4} \approx 0.7853981634 $
- $ \frac{\ln 2}{2} \approx 0.346573590