Let's calculate the integral:

\[
I = \int_1^2 \frac{9x + 4}{x^5 + 3x^2 + x} \, dx
\]

## Step 1: Factor the denominator

First, factor \( x^5 + 3x^2 + x \):

\[
x^5 + 3x^2 + x = x(x^4 + 3x + 1)
\]

## Step 2: Partial Fraction Decomposition

We want to write the integrand as:

\[
\frac{9x+4}{x(x^4 + 3x + 1)} = \frac{A}{x} + \frac{Bx^3 + Cx^2 + Dx + E}{x^4 + 3x + 1}
\]

Multiply both sides by the denominator:

\[
9x + 4 = A(x^4 + 3x + 1) + (Bx^3 + Cx^2 + Dx + E)x
\]
\[
9x + 4 = A x^4 + 3A x + A + Bx^4 + Cx^3 + Dx^2 + Ex
\]

Group by powers of \( x \):

- \( x^4 \): \( A + B \)
- \( x^3 \): \( C \)
- \( x^2 \): \( D \)
- \( x^1 \): \( 3A + E \)
- Constants: \( A \)

Now, set the coefficients equal to those on the left (\( 9x + 4 \)), so:

- \( x^4 \): \( A + B = 0 \implies B = -A \)
- \( x^3 \): \( C = 0 \)
- \( x^2 \): \( D = 0 \)
- \( x^1 \): \( 3A + E = 9 \)
- Constants: \( A = 4 \)

Thus:

- \( A = 4 \)
- \( B = -4 \)
- \( C = 0 \)
- \( D = 0 \)
- \( E = 9 - 3A = 9 - 12 = -3 \)

So,

\[
\frac{9x + 4}{x^5 + 3x^2 + x} = \frac{4}{x} + \frac{-4x^3 - 3}{x^4 + 3x + 1}
\]

## Step 3: Integrate Term by Term

So,

\[
I = \int_1^2 \left[ \frac{4}{x} + \frac{-4x^3 - 3}{x^4 + 3x + 1}\right] dx
\]

Split the integral:

\[
I = \int_1^2 \frac{4}{x} dx - \int_1^2 \frac{4x^3 + 3}{x^4 + 3x + 1} dx
\]

### The first term:

\[
\int_1^2 \frac{4}{x} dx = 4 \int_1^2 \frac{1}{x} dx = 4[\ln x]_1^2 = 4(\ln 2 - \ln 1) = 4 \ln 2
\]

### The second term

\[
\int_1^2 \frac{4x^3 + 3}{x^4 + 3x + 1} dx
\]

Notice that the numerator is almost the derivative of the denominator:

\[
\frac{d}{dx} (x^4 + 3x + 1) = 4x^3 + 3
\]

So,

\[
\int \frac{4x^3 + 3}{x^4 + 3x + 1} dx = \ln|x^4 + 3x + 1| + C
\]

Evaluate on \([1, 2]\):

\[
[x^4 + 3x + 1]_{x=2} = 2^4 + 3 \cdot 2 + 1 = 16 + 6 + 1 = 23
\]
\[
[x^4 + 3x + 1]_{x=1} = 1 + 3 + 1 = 5
\]
Therefore,

\[
\int_1^2 \frac{4x^3 + 3}{x^4 + 3x + 1} dx = \ln 23 - \ln 5 = \ln \frac{23}{5}
\]

But our term is negative of this (due to the negative in the decomposition):

\[
- \int_1^2 \frac{4x^3 + 3}{x^4 + 3x + 1} dx = -\ln \frac{23}{5}
\]

## Step 4: Collect the Results

\[
I = 4 \ln 2 - \ln \frac{23}{5} = 4 \ln 2 - (\ln 23 - \ln 5) = 4\ln 2 + \ln 5 - \ln 23
\]

Or,

\[
I = \ln\left( \frac{16 \cdot 5}{23} \right) = \ln\left( \frac{80}{23} \right)
\]

## Step 5: Numerical Approximation

Calculate \( \ln(80/23) \):

- \( 80 / 23 \approx 3.4782608696 \)
- \( \ln(3.4782608696) \approx 1.2471560635 \)

## Step 6: JSON Output

```json
{"answer": "\\ln\\left(\\frac{80}{23}\\right)", "numerical_answer": "1.2471560635"}
```