We wish to evaluate

  I = ∫₀² x^(1−3/2) · (2−x)^(1−1/2) · [1 − 0.5·x·(2−x)]^(−1) dx.

Step 1. Simplify the Integral

Notice that
  1 − 3/2 = −1/2 and 1 − 1/2 = 1/2.
Thus,
  I = ∫₀² x^(−1/2) (2 − x)^(1/2) [1 − 0.5·x·(2 − x)]^(−1) dx.

Step 2. Substitute x = 2 sin²θ

Let
  x = 2 sin²θ  ⟹ dx = 4 sinθ cosθ dθ.
When x = 0, sinθ = 0 so θ = 0;
when x = 2, sin²θ = 1 so θ = π/2.

Now,
  x^(−1/2) = (2 sin²θ)^(−1/2) = 1/(√2 sinθ),
  (2 − x)^(1/2) = [2 − 2 sin²θ]^(1/2) = (2 cos²θ)^(1/2) = √2 cosθ.
Multiplying these gives:
  x^(−1/2)(2 − x)^(1/2) = (1/(√2 sinθ)) · (√2 cosθ) = cosθ/sinθ.

Also, the dx factor brings 4 sinθ cosθ dθ so:
  [x^(−1/2)(2 − x)^(1/2)] dx = (cosθ/sinθ) · 4 sinθ cosθ dθ = 4 cos²θ dθ.

Next, rewrite the term in the bracket:
  x(2 − x) = [2 sin²θ][2 cos²θ] = 4 sin²θ cos²θ,
so
  1 − 0.5·x(2 − x) = 1 − 0.5·(4 sin²θ cos²θ) = 1 − 2 sin²θ cos²θ.
Notice that
  sin²θ cos²θ = (¼) sin²2θ,
thus
  1 − 2 sin²θ cos²θ = 1 − (1/2) sin²2θ.
Since the bracket appears raised to −1, we now have
  [1 − 2 sin²θ cos²θ]^(−1) = [1 − (1/2) sin²2θ]^(−1).

Putting everything together, the integral becomes
  I = ∫₀^(π/2) 4 cos²θ · [1 − (1/2) sin²2θ]^(−1) dθ.

Step 3. Change of Variable: u = 2θ

Write cos²θ in terms of u by letting
  u = 2θ  ⇒ dθ = du/2.
When θ = 0, u = 0; when θ = π/2, u = π.
Also, note that cos²θ remains as is and we have
  I = ∫₀^(π) 4 cos²(u/2) · [1 − (1/2) sin²u]^(−1) (du/2) = 2 ∫₀^(π) cos²(u/2) [1 − (1/2) sin²u]^(−1) du.

It is convenient now to use the half-angle formula:
  cos²(u/2) = (1 + cos u)/2.
Thus,
  I = 2∫₀^(π) (1 + cos u)/2 · [1 − (1/2) sin²u]^(−1) du = ∫₀^(π) (1 + cos u) / [1 − (1/2) sin²u] du.

Step 4. Split the Integral

Write
  I = ∫₀^(π) 1/(1 − (1/2) sin²u) du + ∫₀^(π) cos u/(1 − (1/2) sin²u) du.
For the second term, use the substitution w = sin u, so dw = cos u du; the limits become 0 at both u = 0 and u = π. Thus, the second integral vanishes. Hence,
  I = ∫₀^(π) 1/(1 − (1/2) sin²u) du.

Step 5. Simplify the Denominator

Write the denominator in a common form:
  1 − (1/2) sin²u = (2 − sin²u)/2.
Thus,
  I = ∫₀^(π) 2/(2 − sin²u) du = 2∫₀^(π) du/(2 − sin²u).

Since sin²u is symmetric about π/2, we have
  ∫₀^(π) du/(2 − sin²u) = 2∫₀^(π/2) du/(2 − sin²u).
Therefore,
  I = 2·2∫₀^(π/2) du/(2 − sin²u) = 4∫₀^(π/2) du/(2 − sin²u).

Step 6. Use a Standard Integral Formula

A standard result is
  ∫₀^(π/2) du/(a − b sin²u) = π/(2√(a(a − b)))  for a > b > 0.
Here, a = 2 and b = 1 so that a − b = 1. Hence,
  ∫₀^(π/2) du/(2 − sin²u) = π/(2√(2·1)) = π/(2√2).

Thus, the original integral becomes
  I = 4 · [π/(2√2)] = (2π)/√2 = π√2.

Step 7. Numerical Approximation

We have
  π√2 ≈ 3.1415926536 × 1.4142135624 ≈ 4.4428829382.

Step 8. Final Answer in JSON Format

{"answer": "$\\sqrt{2}\\pi$", "numerical_answer": "4.4428829382"}