To solve the definite integral \(\int_0^1 \sqrt[4]{\frac{1}{x} - 1} \, dx\), we will follow the steps outlined:

### Step 1: Analytical Solution

First, let's make a substitution to simplify the integral. Let:
\[ u = \sqrt[4]{\frac{1}{x} - 1} \]

Then:
\[ u^4 = \frac{1}{x} - 1 \]
\[ \frac{1}{x} = u^4 + 1 \]
\[ x = \frac{1}{u^4 + 1} \]

Next, we need to find \( dx \) in terms of \( du \):
\[ dx = \frac{d}{du} \left( \frac{1}{u^4 + 1} \right) du \]
\[ dx = -\frac{4u^3}{(u^4 + 1)^2} du \]

Now, substitute \( x \) and \( dx \) back into the integral:
\[ \int_0^1 \sqrt[4]{\frac{1}{x} - 1} \, dx = \int_{u(0)}^{u(1)} u \left( -\frac{4u^3}{(u^4 + 1)^2} \right) du \]

Determine the limits of integration in terms of \( u \):
- When \( x = 0 \), \( u = \sqrt[4]{\frac{1}{0} - 1} \) which is undefined, but we can consider the limit as \( x \to 0^+ \), \( u \to \infty \).
- When \( x = 1 \), \( u = \sqrt[4]{\frac{1}{1} - 1} = 0 \).

So the integral becomes:
\[ \int_{\infty}^{0} u \left( -\frac{4u^3}{(u^4 + 1)^2} \right) du \]

Reversing the limits of integration:
\[ \int_{0}^{\infty} \frac{4u^4}{(u^4 + 1)^2} du \]

### Step 2: Simplify the Integral

We can simplify the integrand:
\[ \frac{4u^4}{(u^4 + 1)^2} = 4 \cdot \frac{u^4}{(u^4 + 1)^2} \]

This integral is a standard form that can be evaluated using partial fractions or known results. The integral evaluates to:
\[ \int_{0}^{\infty} \frac{4u^4}{(u^4 + 1)^2} du = \frac{\pi}{2} \]

### Step 3: Numerical Approximation

The exact answer is \(\frac{\pi}{2}\). To provide a numerical approximation:
\[ \frac{\pi}{2} \approx 1.5707963267948966 \]

### Step 4: Output the Final Answer in JSON Format

```json
{"answer": "\\frac{\\pi}{2}", "numerical_answer": "1.5707963268"}
```