We wish to evaluate

  I = ∫₀^(2π) |1 + 2 sin x| dx.

Step 1. Find the points where the expression changes sign.

Solve 1 + 2 sin x = 0:
  2 sin x = -1 ⟹ sin x = -½.
In [0, 2π] this happens at
  x = 7π/6 and x = 11π/6.

For x in [0, 7π/6] and [11π/6, 2π] we have 1 + 2 sin x ≥ 0, and for x in [7π/6, 11π/6] we have 1 + 2 sin x ≤ 0.

Step 2. Split the integral into three parts:

  I = ∫₀^(7π/6) (1 + 2 sin x) dx + ∫_(7π/6)^(11π/6) |1 + 2 sin x| dx + ∫_(11π/6)^(2π) (1 + 2 sin x) dx.

Since 1 + 2 sin x is negative on [7π/6, 11π/6], we write that part as the negative of the integral of (1 + 2 sin x) over that interval. Thus,

  I = ∫₀^(7π/6) (1 + 2 sin x) dx - ∫_(7π/6)^(11π/6) (1 + 2 sin x) dx + ∫_(11π/6)^(2π) (1 + 2 sin x) dx.

Step 3. Find the antiderivative.

An antiderivative for (1 + 2 sin x) is:
  F(x) = x - 2 cos x.

Now we evaluate each part.

Part A (from 0 to 7π/6):
  A = F(7π/6) - F(0)
    = [7π/6 - 2 cos(7π/6)] - [0 - 2 cos 0]
    = 7π/6 - 2 cos(7π/6) + 2 cos 0.
Since cos(7π/6) = -√3/2 and cos 0 = 1:
  A = 7π/6 - 2 ( -√3/2 ) + 2(1)
    = 7π/6 + √3 + 2.

Part B (from 7π/6 to 11π/6):
  B = F(11π/6) - F(7π/6)
    = [11π/6 - 2 cos(11π/6)] - [7π/6 - 2 cos(7π/6)]
    = (11π/6 - 7π/6) - 2[cos(11π/6) - cos(7π/6)]
    = (4π/6) - 2[cos(11π/6) - cos(7π/6)]
    = (2π/3) - 2[cos(11π/6) - cos(7π/6)].
Now, cos(11π/6) = cos(π/6) = √3/2 and cos(7π/6) = -cos(π/6) = -√3/2. Therefore,
  cos(11π/6) - cos(7π/6) = (√3/2) - ( -√3/2 ) = √3.
Thus,
  B = (2π/3) - 2√3.
Because the function is negative on this interval, its contribution to I is minus B:
  Contribution from Part B = -B = - (2π/3 - 2√3) = 2√3 - 2π/3.

Part C (from 11π/6 to 2π):
  C = F(2π) - F(11π/6)
    = [2π - 2 cos 2π] - [11π/6 - 2 cos(11π/6)]
    = [2π - 2(1)] - [11π/6 - 2 (√3/2)]
    = (2π - 2) - [11π/6 - √3]
    = 2π - 2 - 11π/6 + √3.
Write 2π as 12π/6:
  C = (12π/6 - 11π/6) + √3 - 2
    = (π/6) + √3 - 2.

Step 4. Sum all parts:

  I = A + (Contribution from B) + C
    = [7π/6 + √3 + 2] + [2√3 - 2π/3] + [π/6 + √3 - 2].

Combine the π terms:
  7π/6 + ( - 2π/3 ) + π/6 = 7π/6 + π/6 - 2π/3 = (8π/6) - (4π/6) = 4π/6 = 2π/3.

Combine the √3 terms:
  √3 + 2√3 + √3 = 4√3.

Combine the constant terms:
  2 - 2 = 0.

Thus, the exact result is:
  I = 2π/3 + 4√3.

Step 5. Numerical approximation:

Calculate 2π/3:
  2π/3 ≈ 2 × 3.141592653589793 / 3 ≈ 2.0943951023931953.
Calculate 4√3:
  4√3 ≈ 4 × 1.7320508075688772 ≈ 6.928203230275509.
So the sum is approximately:
  I ≈ 2.0943951023931953 + 6.928203230275509 ≈ 9.022598332668704.
Rounded to 10 decimal places, I ≈ 9.0225983327.

Final answer in JSON format:
{"answer": "\\frac{2\\pi}{3}+4\\sqrt{3}", "numerical_answer": "9.0225983327"}