We start with the integral

  I = ∫₀¹ (x – 1)² (x + 1)² (x² + 1)² (x⁴ + 1)² dx.

Step 1. Notice that
  (x – 1)² (x + 1)² = (x² – 1)².
Then the integrand becomes
  (x² – 1)² (x² + 1)² (x⁴ + 1)².

Step 2. Combine the first two factors:
  (x² – 1)² (x² + 1)² = [(x² – 1)(x² + 1)]² = (x⁴ – 1)².
Thus, the integrand simplifies to
  (x⁴ – 1)² (x⁴ + 1)².

Step 3. Now, note that
  (x⁴ – 1)(x⁴ + 1) = x⁸ – 1.
So,
  (x⁴ – 1)² (x⁴ + 1)² = (x⁸ – 1)².

Since squaring removes the sign, we can write
  (x⁸ – 1)² = (1 – x⁸)².

Step 4. Expand the integrand:
  (1 – x⁸)² = 1 – 2x⁸ + x¹⁶.
Then the integral becomes
  I = ∫₀¹ (1 – 2x⁸ + x¹⁶) dx.

Step 5. Integrate term‐by-term:
  ∫₀¹ 1 dx = 1,
  ∫₀¹ 2x⁸ dx = 2/9,
  ∫₀¹ x¹⁶ dx = 1/17.
Thus,
  I = 1 – 2/9 + 1/17.

Step 6. Combine the fractions using a common denominator. Write
  1 = 153/153,
  2/9 = 34/153 (since 2/9 = (2×17)/(9×17) = 34/153),
  1/17 = 9/153 (since 1/17 = (1×9)/(17×9) = 9/153).
Therefore,
  I = (153 – 34 + 9)/153 = 128/153.

Step 7. Numerical approximation:
  128/153 ≈ 0.8369934641.

The final result is provided in the JSON format below.

{"answer": "\\frac{128}{153}", "numerical_answer": "0.8369934641"}