To solve the definite integral \(\int_{-1/2}^{1/2} \frac{dx}{1 - x^2}\), we will follow the steps outlined:

### Step 1: Compute the Integral Analytically

The integrand \(\frac{1}{1 - x^2}\) can be decomposed using partial fractions. We know that:
\[
\frac{1}{1 - x^2} = \frac{1}{(1 - x)(1 + x)}
\]
We can decompose this into partial fractions:
\[
\frac{1}{(1 - x)(1 + x)} = \frac{A}{1 - x} + \frac{B}{1 + x}
\]
Multiplying both sides by \((1 - x)(1 + x)\) gives:
\[
1 = A(1 + x) + B(1 - x)
\]
To find \(A\) and \(B\), we can set up the following system of equations by equating coefficients:
\[
1 = A + B + (A - B)x
\]
This implies:
\[
A + B = 1 \quad \text{and} \quad A - B = 0
\]
Solving these equations, we get:
\[
A = B = \frac{1}{2}
\]
Thus, the partial fraction decomposition is:
\[
\frac{1}{1 - x^2} = \frac{1/2}{1 - x} + \frac{1/2}{1 + x}
\]
Now, we can integrate each term separately:
\[
\int \frac{1}{1 - x^2} \, dx = \frac{1}{2} \int \frac{1}{1 - x} \, dx + \frac{1}{2} \int \frac{1}{1 + x} \, dx
\]
These integrals are standard:
\[
\int \frac{1}{1 - x} \, dx = -\ln|1 - x| + C_1
\]
\[
\int \frac{1}{1 + x} \, dx = \ln|1 + x| + C_2
\]
Combining these results, we get:
\[
\int \frac{1}{1 - x^2} \, dx = \frac{1}{2} \left( -\ln|1 - x| + \ln|1 + x| \right) + C
\]
Simplifying, we have:
\[
\int \frac{1}{1 - x^2} \, dx = \frac{1}{2} \ln \left| \frac{1 + x}{1 - x} \right| + C
\]

### Step 2: Evaluate the Definite Integral

Now, we evaluate the definite integral from \(-1/2\) to \(1/2\):
\[
\int_{-1/2}^{1/2} \frac{1}{1 - x^2} \, dx = \left[ \frac{1}{2} \ln \left| \frac{1 + x}{1 - x} \right| \right]_{-1/2}^{1/2}
\]
Evaluating at the upper limit \(x = 1/2\):
\[
\frac{1}{2} \ln \left| \frac{1 + 1/2}{1 - 1/2} \right| = \frac{1}{2} \ln \left| \frac{3/2}{1/2} \right| = \frac{1}{2} \ln 3
\]
Evaluating at the lower limit \(x = -1/2\):
\[
\frac{1}{2} \ln \left| \frac{1 - 1/2}{1 + 1/2} \right| = \frac{1}{2} \ln \left| \frac{1/2}{3/2} \right| = \frac{1}{2} \ln \left( \frac{1}{3} \right) = -\frac{1}{2} \ln 3
\]
Subtracting these results:
\[
\frac{1}{2} \ln 3 - \left( -\frac{1}{2} \ln 3 \right) = \frac{1}{2} \ln 3 + \frac{1}{2} \ln 3 = \ln 3
\]

### Step 3: Numerical Approximation

The numerical approximation of \(\ln 3\) to 10 decimal places is:
\[
\ln 3 \approx 1.0986122887
\]

### Step 4: Output the Final Answer in JSON Format

\[
\boxed{
\begin{aligned}
&\text{"answer": "\ln 3",} \\
&\text{"numerical_answer": "1.0986122887"}
\end{aligned}
}
\]