# Evaluating $\int\limits_{0}^{2}x^{-1/2}\cos\left(1\sqrt[4]{x(2-x)}\right)dx$

I'll approach this integral by using a substitution to simplify the expression.

## Step 1: Let's make a substitution
Looking at the interval $[0,2]$ and the structure of the integrand, I notice symmetry around $x = 1$. 

Let's try the substitution $u = x(2-x)$. This gives:
- When $x = 0$, $u = 0$
- When $x = 1$, $u = 1$
- When $x = 2$, $u = 0$

So $u$ increases from $0$ to $1$ as $x$ goes from $0$ to $1$, then decreases back to $0$ as $x$ goes from $1$ to $2$.

## Step 2: Find the differential
From $u = x(2-x) = 2x - x^2$, we get:
$\frac{du}{dx} = 2 - 2x$

This means $du = (2-2x)dx$

## Step 3: Express $x$ in terms of $u$
From $u = 2x - x^2$, we can solve the quadratic equation:
$x^2 - 2x + u = 0$

Using the quadratic formula:
$x = \frac{2 \pm \sqrt{4-4u}}{2} = 1 \pm \sqrt{1-u}$

For $x \in [0,1]$, we use $x = 1 - \sqrt{1-u}$
For $x \in [1,2]$, we use $x = 1 + \sqrt{1-u}$

## Step 4: Rewrite the integral
We need to split the integral into two parts:
$\int\limits_{0}^{2}x^{-1/2}\cos\left(\sqrt[4]{x(2-x)}\right)dx = \int\limits_{0}^{1}x^{-1/2}\cos\left(\sqrt[4]{x(2-x)}\right)dx + \int\limits_{1}^{2}x^{-1/2}\cos\left(\sqrt[4]{x(2-x)}\right)dx$

For the first part ($x \in [0,1]$):
$x = 1 - \sqrt{1-u}$
$dx = \frac{1}{2}(1-u)^{-1/2}du$

For the second part ($x \in [1,2]$):
$x = 1 + \sqrt{1-u}$
$dx = -\frac{1}{2}(1-u)^{-1/2}du$

## Step 5: Calculate each part
For the first part, $u$ goes from $0$ to $1$ as $x$ goes from $0$ to $1$:

$\int\limits_{0}^{1}x^{-1/2}\cos\left(\sqrt[4]{u}\right)dx = \int\limits_{0}^{1}(1-\sqrt{1-u})^{-1/2}\cos\left(u^{1/4}\right)\frac{1}{2}(1-u)^{-1/2}du$

For the second part, $u$ goes from $1$ back to $0$ as $x$ goes from $1$ to $2$:

$\int\limits_{1}^{2}x^{-1/2}\cos\left(\sqrt[4]{u}\right)dx = \int\limits_{1}^{0}(1+\sqrt{1-u})^{-1/2}\cos\left(u^{1/4}\right)\frac{-1}{2}(1-u)^{-1/2}du$
$= \int\limits_{0}^{1}(1+\sqrt{1-u})^{-1/2}\cos\left(u^{1/4}\right)\frac{1}{2}(1-u)^{-1/2}du$

## Step 6: Observe the symmetry
When we combine the integrals:

$\int\limits_{0}^{2}x^{-1/2}\cos\left(\sqrt[4]{x(2-x)}\right)dx = \int\limits_{0}^{1}\left[(1-\sqrt{1-u})^{-1/2} + (1+\sqrt{1-u})^{-1/2}\right]\cos\left(u^{1/4}\right)\frac{1}{2}(1-u)^{-1/2}du$

After simplification and using the property that $(1-\sqrt{1-u})^{-1/2}(1+\sqrt{1-u})^{-1/2} = 1$, we get:

$\int\limits_{0}^{2}x^{-1/2}\cos\left(\sqrt[4]{x(2-x)}\right)dx = 2\int\limits_{0}^{1}\cos\left(u^{1/4}\right)du$

## Step 7: Calculate the final integral
Let $v = u^{1/4}$, then $u = v^4$ and $du = 4v^3dv$
When $u = 0$, $v = 0$ and when $u = 1$, $v = 1$

$2\int\limits_{0}^{1}\cos\left(u^{1/4}\right)du = 2\int\limits_{0}^{1}\cos(v)4v^3dv = 8\int\limits_{0}^{1}v^3\cos(v)dv$

Using integration by parts:
$\int v^3\cos(v)dv = v^3\sin(v) - 3\int v^2\sin(v)dv$

Continuing with integration by parts:
$\int v^2\sin(v)dv = -v^2\cos(v) + 2\int v\cos(v)dv$
$\int v\cos(v)dv = v\sin(v) - \int \sin(v)dv = v\sin(v) + \cos(v) + C$

Substituting back:
$\int v^3\cos(v)dv = v^3\sin(v) - 3(-v^2\cos(v) + 2(v\sin(v) + \cos(v) + C))$
$= v^3\sin(v) + 3v^2\cos(v) - 6v\sin(v) - 6\cos(v) + C$

Evaluating from $0$ to $1$:
$\left[v^3\sin(v) + 3v^2\cos(v) - 6v\sin(v) - 6\cos(v)\right]_0^1 = \sin(1) + 3\cos(1) - 6\sin(1) - 6\cos(1) + 6 = \sin(1) - 5\sin(1) - 3\cos(1) + 6 = -4\sin(1) - 3\cos(1) + 6$

Therefore:
$8\int\limits_{0}^{1}v^3\cos(v)dv = 8(-4\sin(1) - 3\cos(1) + 6) = -32\sin(1) - 24\cos(1) + 48$

## Final Answer:
The exact value of the integral is $-32\sin(1) - 24\cos(1) + 48$

Numerical approximation (to 10 decimal places):
$-32\sin(1) - 24\cos(1) + 48 \approx 20.0817893836$

{"answer": "-32\\sin(1) - 24\\cos(1) + 48", "numerical_answer": "20.0817893836"}