

To solve the definite integral \(\int_0^1 \frac{\ln\left(x + x^{-1}\right)}{x + x^{-1}} \, dx\), we proceed as follows:

### Step 1: Simplify the integrand
First, rewrite \(x + x^{-1}\) as \(\frac{x^2 + 1}{x}\). The integrand becomes:
\[
\frac{\ln\left(\frac{x^2 + 1}{x}\right)}{\frac{x^2 + 1}{x}} = \frac{x \ln\left(\frac{x^2 + 1}{x}\right)}{x^2 + 1} = \frac{x \ln(x^2 + 1) - x \ln x}{x^2 + 1}.
\]
Thus, the integral splits into two parts:
\[
I = \int_0^1 \frac{x \ln(x^2 + 1)}{x^2 + 1} \, dx - \int_0^1 \frac{x \ln x}{x^2 + 1} \, dx = I_1 - I_2.
\]

### Step 2: Evaluate \(I_1\)
For \(I_1 = \int_0^1 \frac{x \ln(x^2 + 1)}{x^2 + 1} \, dx\), use the substitution \(u = x^2 + 1\), so \(du = 2x \, dx\) (i.e., \(x \, dx = \frac{du}{2}\)). When \(x = 0\), \(u = 1\); when \(x = 1\), \(u = 2\). Thus:
\[
I_1 = \frac{1}{2} \int_1^2 \frac{\ln u}{u} \, du.
\]
The integral \(\int \frac{\ln u}{u} \, du = \frac{1}{2} (\ln u)^2 + C\). Evaluating from \(1\) to \(2\):
\[
I_1 = \frac{1}{2} \left[ \frac{(\ln 2)^2}{2} - \frac{(\ln 1)^2}{2} \right] = \frac{(\ln 2)^2}{4}.
\]

### Step 3: Evaluate \(I_2\)
For \(I_2 = \int_0^1 \frac{x \ln x}{x^2 + 1} \, dx\), use the substitution \(t = x^2\), so \(dt = 2x \, dx\) (i.e., \(x \, dx = \frac{dt}{2}\)) and \(\ln x = \frac{1}{2} \ln t\). When \(x = 0\), \(t = 0\); when \(x = 1\), \(t = 1\). Thus:
\[
I_2 = \frac{1}{4} \int_0^1 \frac{\ln t}{t + 1} \, dt.
\]
The integral \(\int_0^1 \frac{\ln t}{t + 1} \, dt\) can be expanded using the power series \(\frac{1}{t + 1} = \sum_{n=0}^\infty (-1)^n t^n\) (valid for \(|t| < 1\)). Integrating term-by-term:
\[
\int_0^1 \frac{\ln t}{t + 1} \, dt = \sum_{n=0}^\infty (-1)^n \int_0^1 t^n \ln t \, dt.
\]
The integral \(\int_0^1 t^n \ln t \, dt = -\frac{1}{(n + 1)^2}\). Thus:
\[
\int_0^1 \frac{\ln t}{t + 1} \, dt = -\sum_{n=0}^\infty \frac{(-1)^n}{(n + 1)^2} = -\eta(2),
\]
where \(\eta(2)\) is the Dirichlet eta function. Since \(\eta(2) = \frac{\pi^2}{12}\), we have:
\[
\int_0^1 \frac{\ln t}{t + 1} \, dt = -\frac{\pi^2}{12}.
\]
Thus, \(I_2 = \frac{1}{4} \left(-\frac{\pi^2}{12}\right) = -\frac{\pi^2}{48}\).

### Step 4: Combine results
The original integral is:
\[
I = I_1 - I_2 = \frac{(\ln 2)^2}{4} - \left(-\frac{\pi^2}{48}\right) = \frac{(\ln 2)^2}{4} + \frac{\pi^2}{48}.
\]

### Numerical Approximation
- \((\ln 2)^2 \approx 0.4804530139\), so \(\frac{(\ln 2)^2}{4} \approx 0.1201132535\).
- \(\pi^2 \approx 9.8696044011\), so \(\frac{\pi^2}{48} \approx 0.2056167584\).
- Adding these: \(0.1201132535 + 0.2056167584 \approx 0.3257300119\).

Rounded to 10 decimal places, the numerical approximation is \(0.3257300119\).

{"answer": "\\frac{(\\ln 2)^2}{4} + \\frac{\\pi^2}{48}", "numerical_answer": "0.3257300119"}