Let's compute the integral:
\[
\int_0^6 x + (x-3)^7 + \sin(x-3) \, dx
\]

**Step 1: Integrate analytically (find the antiderivative)**

We can split the integral:
\[
\int_0^6 x \, dx + \int_0^6 (x-3)^7 dx + \int_0^6 \sin(x-3) dx
\]

Compute each term:

1. \(\int_0^6 x \, dx = \left. \frac{x^2}{2} \right|_0^6 = \frac{36}{2} - 0 = 18\)

2. For \(\int_0^6 (x-3)^7 dx\), use substitution: \(u = x - 3\) \(\implies x = u+3\), when \(x = 0, u = -3\), when \(x = 6, u = 3\):
   \[
   \int_0^6 (x-3)^7 dx = \int_{-3}^{3} u^7 du = \left. \frac{u^8}{8} \right|_{-3}^{3}
   \]
   Since \(u^8\) is even, \(u^8|_{-3}^{3} = (3^8) - ((-3)^8) = 0\), since both terms are equal:
   \[
   \frac{3^8 - (-3)^8}{8} = \frac{6561 - 6561}{8} = 0
   \]
   So this integral is \(0\).

3. For \(\int_0^6 \sin(x-3) dx\), again substitute \(u=x-3\), so as before, as \(x\) goes from \(0\) to \(6\), \(u\) goes from \(-3\) to \(3\):
   \[
   \int_0^6 \sin(x-3) dx = \int_{-3}^{3} \sin u \, du = -\cos u \bigg|_{-3}^{3} = -\cos(3) + \cos(-3)
   \]
   But \(\cos(-3) = \cos(3)\), so the difference is zero:
   \[
   -\cos(3) + \cos(3) = 0
   \]
   So this integral is \(0\).

**Step 2: Sum all terms**

\[
18 + 0 + 0 = 18
\]

**Step 3: Numerical approximation**

\[
18 \text{ (rounded to 10 decimal places: 18.0000000000)}
\]

**Step 4: JSON output**

```json
{"answer": "18", "numerical_answer": "18.0000000000"}
```