# Evaluating $\int_0^{\frac{\pi}{4}}\tan^{-1}\left(\frac{1+\tan(x)}{\sqrt{2}}\right)\mathrm{d}x$

## Step 1: Let's make a substitution to simplify
Let $t = \tan(x)$, then $dx = \frac{dt}{1+t^2}$ and when $x = 0$, $t = 0$, and when $x = \frac{\pi}{4}$, $t = 1$.

The integral becomes:
$$\int_0^{1}\tan^{-1}\left(\frac{1+t}{\sqrt{2}}\right)\frac{dt}{1+t^2}$$

## Step 2: Let's analyze the expression $\frac{1+t}{\sqrt{2}}$
First, note that:
$$\tan^{-1}\left(\frac{1+t}{\sqrt{2}}\right) = \tan^{-1}\left(\frac{1}{\sqrt{2}} + \frac{t}{\sqrt{2}}\right)$$

## Step 3: Make another substitution
Let $u = \frac{1+t}{\sqrt{2}}$, then $t = \sqrt{2}u - 1$ and $dt = \sqrt{2}du$.

When $t = 0$, $u = \frac{1}{\sqrt{2}}$, and when $t = 1$, $u = \frac{2}{\sqrt{2}} = \sqrt{2}$.

The integral becomes:
$$\int_{\frac{1}{\sqrt{2}}}^{\sqrt{2}}\tan^{-1}(u)\frac{\sqrt{2}du}{1+(\sqrt{2}u-1)^2}$$

## Step 4: Simplify the denominator
$$1+(\sqrt{2}u-1)^2 = 1+2u^2-2\sqrt{2}u+1 = 2+2u^2-2\sqrt{2}u$$

We can rewrite this as:
$$2+2u^2-2\sqrt{2}u = 2(1+u^2-\sqrt{2}u) = 2(1+u^2-\sqrt{2}u+\frac{2}{2}-\frac{2}{2}) = 2(1+u^2-\sqrt{2}u+1-1)$$

$$= 2(2+u^2-\sqrt{2}u-1) = 2(1+(u-\frac{\sqrt{2}}{2})^2) = 2(1+(u-\frac{1}{\sqrt{2}})^2)$$

## Step 5: Continue with substitution
Let $v = u-\frac{1}{\sqrt{2}}$, then $du = dv$.
When $u = \frac{1}{\sqrt{2}}$, $v = 0$, and when $u = \sqrt{2}$, $v = \sqrt{2}-\frac{1}{\sqrt{2}} = \frac{2-1}{\sqrt{2}} = \frac{1}{\sqrt{2}}$.

Our integral becomes:
$$\int_{0}^{\frac{1}{\sqrt{2}}}\tan^{-1}(v+\frac{1}{\sqrt{2}})\frac{\sqrt{2}dv}{2(1+v^2)} = \frac{1}{\sqrt{2}}\int_{0}^{\frac{1}{\sqrt{2}}}\tan^{-1}(v+\frac{1}{\sqrt{2}})\frac{dv}{1+v^2}$$

## Step 6: Using properties of inverse tangent
We can use the identity:
$$\tan^{-1}(a) + \tan^{-1}(b) = \tan^{-1}\left(\frac{a+b}{1-ab}\right) \quad \text{for } ab < 1$$

For our case, we have:
$$\tan^{-1}(v+\frac{1}{\sqrt{2}}) = \tan^{-1}(v) + \tan^{-1}(\frac{1}{\sqrt{2}}) - \pi \cdot I$$

Where $I = 0$ if $(v)(1/\sqrt{2}) < 1$ and $I = \text{sgn}(v)$ if $(v)(1/\sqrt{2}) > 1$.

In our case, for $v \in [0, 1/\sqrt{2}]$, we always have $(v)(1/\sqrt{2}) < 1$, so $I = 0$.

Thus:
$$\tan^{-1}(v+\frac{1}{\sqrt{2}}) = \tan^{-1}(v) + \tan^{-1}(\frac{1}{\sqrt{2}})$$

And $\tan^{-1}(\frac{1}{\sqrt{2}}) = \frac{\pi}{8}$ (since $\tan(\frac{\pi}{8}) = \frac{1}{\sqrt{2}}-1$).

## Step 7: Simplify the integral
Our integral becomes:
$$\frac{1}{\sqrt{2}}\int_{0}^{\frac{1}{\sqrt{2}}}(\tan^{-1}(v) + \frac{\pi}{8})\frac{dv}{1+v^2}$$

$$= \frac{1}{\sqrt{2}}\int_{0}^{\frac{1}{\sqrt{2}}}\tan^{-1}(v)\frac{dv}{1+v^2} + \frac{1}{\sqrt{2}} \cdot \frac{\pi}{8}\int_{0}^{\frac{1}{\sqrt{2}}}\frac{dv}{1+v^2}$$

For the first integral, we can use the formula:
$$\int \tan^{-1}(v)\frac{dv}{1+v^2} = \frac{1}{2}(\tan^{-1}(v))^2 + C$$

For the second integral:
$$\int \frac{dv}{1+v^2} = \tan^{-1}(v) + C$$

## Step 8: Evaluate the limits
$$\frac{1}{\sqrt{2}}\left[\frac{1}{2}(\tan^{-1}(v))^2 + \frac{\pi}{8}\tan^{-1}(v)\right]_{0}^{\frac{1}{\sqrt{2}}}$$

$$= \frac{1}{\sqrt{2}}\left[\frac{1}{2}(\tan^{-1}(\frac{1}{\sqrt{2}}))^2 + \frac{\pi}{8}\tan^{-1}(\frac{1}{\sqrt{2}}) - \frac{1}{2}(\tan^{-1}(0))^2 - \frac{\pi}{8}\tan^{-1}(0)\right]$$

$$= \frac{1}{\sqrt{2}}\left[\frac{1}{2}(\frac{\pi}{8})^2 + \frac{\pi}{8} \cdot \frac{\pi}{8} - 0 - 0\right]$$

$$= \frac{1}{\sqrt{2}}\left[\frac{1}{2} \cdot \frac{\pi^2}{64} + \frac{\pi^2}{64}\right] = \frac{1}{\sqrt{2}} \cdot \frac{3\pi^2}{128} = \frac{3\pi^2}{128\sqrt{2}}$$

## Step 9: Final simplification
$$\frac{3\pi^2}{128\sqrt{2}} = \frac{3\pi^2}{128 \cdot \sqrt{2}} \cdot \frac{\sqrt{2}}{\sqrt{2}} = \frac{3\pi^2\sqrt{2}}{256}$$

## Step 10: Numerical approximation
$\frac{3\pi^2\sqrt{2}}{256} \approx 0.1298804780$

Therefore, the definite integral equals $\frac{3\pi^2\sqrt{2}}{256}$.

{"answer": "\\frac{3\\pi^2\\sqrt{2}}{256}", "numerical_answer": "0.1298804780"}