<think>
Okay, let's see. I need to compute the definite integral from -1 to 1 of sin(sqrt(x)) divided by [sinh(sqrt(x)) + sin(sqrt(x))] dx. Hmm, that looks a bit tricky. First, I should check if the function is defined over the interval. Wait, the square root of x is only real for x ≥ 0. But the integral is from -1 to 1. So, for x between -1 and 0, sqrt(x) would be imaginary. That complicates things. Maybe there's a substitution or symmetry here?

Let me think. The integrand is sin(sqrt(x))/(sinh(sqrt(x)) + sin(sqrt(x))). For x negative, sqrt(x) is i*sqrt(|x|), right? So, let's substitute x = -t where t is positive. Then, when x is from -1 to 0, t is from 0 to 1. Let's split the integral into two parts: from -1 to 0 and 0 to 1.

So, integral = ∫_{-1}^0 ... dx + ∫_{0}^1 ... dx.

For the first integral, let x = -t, so dx = -dt. Then, when x = -1, t = 1; x=0, t=0. So the first integral becomes ∫_{1}^{0} [sin(sqrt(-t)) / (sinh(sqrt(-t)) + sin(sqrt(-t)))] (-dt) = ∫_{0}^{1 [sin(i sqrt(t)) / (sinh(i sqrt(t)) + sin(i sqrt(t)))] dt.

But sinh(iz) = i sin(z), and sin(iz) = i sinh(z). Let me recall hyperbolic identities. So, sinh(iy) = i sin(y), and sin(iy) = i sinh(y). So, sqrt(-t) = i sqrt(t). Therefore, sin(sqrt(-t)) = sin(i sqrt(t)) = i sinh(sqrt(t)). Similarly, sinh(sqrt(-t)) = sinh(i sqrt(t)) = i sin(sqrt(t)).

So substituting into the first integral:

sin(sqrt(-t)) / [sinh(sqrt(-t)) + sin(sqrt(-t))] = [i sinh(sqrt(t))] / [i sin(sqrt(t)) + i sinh(sqrt(t))] = [i sinh(sqrt(t))] / [i (sin(sqrt(t)) + sinh(sqrt(t)))] = sinh(sqrt(t)) / (sin(sqrt(t)) + sinh(sqrt(t))).

So the first integral becomes ∫_{0}^{1} [sinh(sqrt(t)) / (sin(sqrt(t)) + sinh(sqrt(t)))] dt.

Now, the original integral is the sum of the first integral (from 0 to1) and the second integral (from 0 to1 of [sin(sqrt(x)) / (sinh(sqrt(x)) + sin(sqrt(x)))] dx). Let me denote the second integral as I = ∫_{0}^{1} [sin(sqrt(x)) / (sinh(sqrt(x)) + sin(sqrt(x)))] dx. Then the first integral is ∫_{0}^{1} [sinh(sqrt(t)) / (sinh(sqrt(t)) + sin(sqrt(t)))] dt. Let's call that J. So the total integral is I + J.

But notice that I and J are integrals over the same interval, and their integrands are sin/(sinh + sin) and sinh/(sinh + sin). So if we add them together, we get ∫_{0}^{1} [sin + sinh]/(sinh + sin) dx = ∫_{0}^{1} 1 dx = 1. Therefore, I + J = 1. Therefore, the original integral from -1 to1 is equal to 1.

Wait, that's brilliant! Because when you split the integral into negative and positive parts, the negative part transforms into an integral that, when added to the positive part, sums up to 1. So the total integral is 1. So the exact answer is 1. Let me check this again.

So, for x in [-1,0], substitution x = -t gives us the integrand sinh(sqrt(t))/(sinh(sqrt(t)) + sin(sqrt(t))). Then, adding the two integrals from 0 to1, the integrands are sin/(sinh + sin) and sinh/(sinh + sin). Adding them gives 1, so the integral from 0 to1 of 1 dt is 1. Therefore, the total integral is 1. That seems correct. So the exact answer is 1. Then, numerically, 1.0000000000. Let me confirm with a numerical approximation. If I compute the integral numerically, it should be 1. Let's test with a simple case. Suppose x=0.25. Then sqrt(x)=0.5. Compute sin(0.5)/(sinh(0.5)+sin(0.5)) + sinh(0.5)/(sinh(0.5)+sin(0.5)) = (sin(0.5) + sinh(0.5))/(sinh(0.5)+sin(0.5)) =1. So for each x in [0,1], the sum of the two terms is 1. Therefore, integrating over [0,1] gives 1. Therefore, the total integral is 1. So the exact answer is 1, and the numerical approximation is 1.0000000000.
</think>

{"answer": "1", "numerical_answer": "1.0000000000"}