Given:
\[
I = \int_0^1 x^{-1/4} (1-x)^{1/4} I_1\left(\sqrt[4]{x(1-x)}\right) \, dx
\]
where \( I_1 \) is the modified Bessel function of the first kind.

Let's solve step by step.

---

**Step 1: Series Expansion for \( I_1 \)**

Recall the power series expansion:
\[
I_1(z) = \sum_{k=0}^\infty \frac{1}{k! \, \Gamma(k+2)} \left(\frac{z}{2}\right)^{2k+1}
\]

Let \( z = (x(1-x))^{1/4} \), so:
\[
I_1(z) = \sum_{k=0}^\infty \frac{1}{k! \Gamma(k+2)} \left(\frac{(x(1-x))^{1/4}}{2}\right)^{2k+1}
= \sum_{k=0}^\infty \frac{1}{k! \Gamma(k+2) 2^{2k+1}} (x(1-x))^{(2k+1)/4}
\]

---

**Step 2: Substitute Series into the Integral**

So the integrand is:
\[
x^{-1/4}(1-x)^{1/4} \cdot (x(1-x))^{(2k+1)/4}
= x^{-1/4 + (2k+1)/4} (1-x)^{1/4 + (2k+1)/4}
= x^{k/2} (1-x)^{(k+1)/2}
\]

So,
\[
I = \int_0^1 x^{-1/4}(1-x)^{1/4} I_1\left((x(1-x))^{1/4}\right) dx
= \sum_{k=0}^\infty \frac{1}{k! \Gamma(k+2) 2^{2k+1}} \int_0^1 x^{k/2} (1-x)^{(k+1)/2} dx
\]

---

**Step 3: Solve the Inner Integral**

The general beta integral is:
\[
\int_0^1 x^{a-1}(1-x)^{b-1} dx = \mathrm{B}(a, b) = \frac{\Gamma(a)\Gamma(b)}{\Gamma(a+b)}
\]

So for our integrand:
- \( a-1 = k/2 \implies a = k/2 + 1 \)
- \( b-1 = (k+1)/2 \implies b = (k+1)/2 + 1 = (k+3)/2 \)

So:
\[
\int_0^1 x^{k/2} (1-x)^{(k+1)/2} dx = \frac{\Gamma(k/2 + 1)\, \Gamma((k+3)/2)}{\Gamma(k/2 + 1 + (k+3)/2)} = \frac{\Gamma(k/2+1)\,\Gamma\left(\frac{k+3}{2}\right)}{\Gamma\left( k+2.5 \right)}
\]

---

**Step 4: Write the Series Representation**

So,
\[
I = \sum_{k=0}^\infty \frac{1}{k!\,\Gamma(k+2)\,2^{2k+1}}
\frac{\Gamma\left(\frac{k}{2}+1\right)\Gamma\left(\frac{k+3}{2}\right)}{\Gamma(k+2.5)}
\]

---

**Can this sum be reduced to elementary functions?**

It doesn't seem to reduce to elementary or classical special functions in closed form. This is a rapidly converging sum.

---

**Step 5: Numerical Evaluation**

Let's compute the first few terms and sum until convergence.

Define:
\[
a_k = \frac{1}{k!\,\Gamma(k+2)\,2^{2k+1}}
\frac{\Gamma\left(\frac{k}{2}+1\right)\Gamma\left(\frac{k+3}{2}\right)}{\Gamma(k+2.5)}
\]

Let's compute several terms:

For \( k = 0 \):
- \( k! = 1 \)
- \( \Gamma(2) = 1 \)
- \( 2^{1} = 2 \)
- \( \Gamma(1) = 1 \)
- \( \Gamma(1.5) = \frac{\sqrt{\pi}}{2} \)
- \( \Gamma(2.5) = \frac{3\sqrt{\pi}}{4} \)

\[
a_0 = \frac{1}{1 \cdot 1 \cdot 2} \cdot \frac{1 \cdot \frac{\sqrt{\pi}}{2}}{ \frac{3\sqrt{\pi}}{4} }
= \frac{1}{2} \cdot \frac{1}{1} \cdot \frac{1}{2} \cdot \frac{4}{3}
= \frac{1}{2} \cdot \frac{4}{6}
= \frac{4}{12}
= \frac{1}{3}
\]

For \( k = 1 \):
- \( k! = 1 \)
- \( \Gamma(3) = 2 \)
- \( 2^3 = 8 \)
- \( \Gamma(1.5) = \frac{\sqrt{\pi}}{2} \)
- \( \Gamma(2) = 1 \)
- \( \Gamma(3.5) = \frac{3 \cdot 1.5 \cdot \sqrt{\pi}}{4} = \frac{9\sqrt{\pi}}{8} \)

\[
a_1 = \frac{1}{1 \cdot 2 \cdot 8} \cdot \frac{ \frac{\sqrt{\pi}}{2} \cdot 1 }{ \frac{9\sqrt{\pi}}{8} }
= \frac{1}{16} \cdot \frac{ \frac{\sqrt{\pi}}{2} }{ \frac{9\sqrt{\pi}}{8} }
= \frac{1}{16} \cdot \frac{8}{18}
= \frac{1}{16} \cdot \frac{4}{9}
= \frac{1}{36}
\]

For \( k = 2 \):
- \( k! = 2 \)
- \( \Gamma(4) = 6 \)
- \( 2^5 = 32 \)
- \( \Gamma(2) = 1 \)
- \( \Gamma(2.5) = \frac{3\sqrt{\pi}}{4} \)
- \( \Gamma(4.5) = \frac{7 \cdot 5 \cdot 3 \cdot 1.5 \cdot \sqrt{\pi}}{16} = \frac{105\sqrt{\pi}}{16} \)

\[
a_2 = \frac{1}{2 \cdot 6 \cdot 32} \cdot \frac{1 \cdot \frac{3\sqrt{\pi}}{4} }{ \frac{105\sqrt{\pi}}{16} }
= \frac{1}{384} \cdot \frac{ 3/4 }{ 105/16 }
= \frac{1}{384} \cdot \frac{3/4 \cdot 16}{105}
= \frac{1}{384} \cdot \frac{48}{420}
= \frac{1}{384} \cdot \frac{12}{105}
= \frac{12}{384 \cdot 105}
= \frac{1}{3360}
\]

For \( k = 3 \):
- \( k! = 6 \)
- \( \Gamma(5) = 24 \)
- \( 2^7 = 128 \)
- \( \Gamma(2.5) = \frac{3\sqrt{\pi}}{4} \)
- \( \Gamma(3) = 2 \)
- \( \Gamma(5.5) = \frac{945\sqrt{\pi}}{32} \)

\[
a_3 = \frac{1}{6 \cdot 24 \cdot 128} \cdot \frac{ \frac{3\sqrt{\pi}}{4} \cdot 2 }{ \frac{945\sqrt{\pi}}{32} }
= \frac{1}{18432} \cdot \frac{ 6 \cdot 32 }{ 4 \cdot 945 }
= \frac{1}{18432} \cdot \frac{192}{3780}
= \frac{1}{18432} \cdot \frac{16}{315}
= \frac{16}{18432 \cdot 315}
= \frac{16}{5806080}
= \frac{1}{363,200}
\]

Now sum up these terms:
- \( a_0 = \frac{1}{3} \approx 0.3333333333 \)
- \( a_1 = \frac{1}{36} \approx 0.0277777778 \)
- \( a_2 = \frac{1}{3360} \approx 0.0002976190 \)
- \( a_3 = \frac{1}{363200} \approx 0.0000027536 \)

Total so far: \( 0.3333333333 + 0.0277777778 + 0.0002976190 + 0.0000027536 \approx 0.3614114837 \)

Now let's see higher-order terms:

\( a_4 \) is much, much smaller. Quickly calculating, the next correction is \(\sim 10^{-8}\) or less.

**Thus, the value converges rapidly to about \( 0.3614114837 \).**

---

**Step 6: Final boxed answers**

**Exact form:**
\[
\boxed{
\int_0^1 x^{-1/4} (1-x)^{1/4} I_1\left( (x(1-x))^{1/4} \right) dx
= \sum_{k=0}^\infty \frac{\Gamma\left( \frac{k}{2} + 1 \right) \Gamma\left( \frac{k+3}{2} \right)}{k!\,\Gamma(k+2)\,2^{2k+1}\,\Gamma(k+2.5)}
}
\]

**Numerical evaluation (10 digits):**
\[
\boxed{0.3614114837}
\]

---

**Step 7: Output as requested in JSON format**
```json
{"answer": "\sum_{k=0}^\infty \\frac{\\Gamma\\left( \\frac{k}{2} + 1 \\right) \\Gamma\\left( \\frac{k+3}{2} \\right)}{k!\\,\\Gamma(k+2)\\,2^{2k+1}\\,\\Gamma(k+2.5)}", "numerical_answer": "0.3614114837"}
```