We wish to evaluate

  I = ∫₀² x H₃(√[x(2–x)]) dx

where H₃ is the (physicists’) Hermite polynomial of degree 3. In our notation

  H₃(z) = 8z³ – 12z.

Thus,
  I = ∫₀² x [8 (√(x(2–x)))³ – 12 √(x(2–x))] dx
    = 8 ∫₀² x (x(2–x))^(3/2) dx – 12 ∫₀² x (x(2–x))^(1/2) dx.

Define the two integrals

  I₁ = ∫₀² x (x(2–x))^(3/2) dx  and  I₂ = ∫₀² x (x(2–x))^(1/2) dx.

Step 1. Express I₁ and I₂ in Beta–integral form.

Notice that
  (x(2–x))^(α) = x^(α)(2–x)^(α).

Thus,
  I₁ = ∫₀² x · [x^(3/2)(2–x)^(3/2)] dx
    = ∫₀² x^(5/2) (2–x)^(3/2) dx,
and
  I₂ = ∫₀² x · [x^(1/2)(2–x)^(1/2)] dx
    = ∫₀² x^(3/2) (2–x)^(1/2) dx.

We now perform the substitution

  x = 2u,  so that dx = 2 du  with u ∈ [0, 1].
Then 2–x = 2–2u = 2(1–u).

For I₁ we have:
  I₁ = ∫₀¹ (2u)^(5/2) [2(1–u)]^(3/2) (2 du)
    = 2^(5/2)  u^(5/2) · 2^(3/2)(1–u)^(3/2) · 2 du
    = 2^(5/2+3/2+1) ∫₀¹ u^(5/2)(1–u)^(3/2) du
    = 2^( (5+3+2)/2 ) ∫₀¹ u^(5/2)(1–u)^(3/2) du
    = 2^(10/2) ∫₀¹ u^(5/2)(1–u)^(3/2) du
    = 2⁵ ∫₀¹ u^(5/2)(1–u)^(3/2) du  = 32 ∫₀¹ u^(5/2)(1–u)^(3/2) du.

Note that the Beta integral is given by 
  B(a, b) = ∫₀¹ u^(a–1)(1–u)^(b–1) du.
Here, writing u^(5/2) = u^((7/2)–1) and (1–u)^(3/2) = (1–u)^((5/2)–1), we have
  a = 7/2 and b = 5/2.
Thus,
  I₁ = 32 B(7/2, 5/2) = 32 · (Γ(7/2)Γ(5/2))/Γ(7/2+5/2)
      = 32 · (Γ(7/2)Γ(5/2))/Γ(6).

Recall:
  Γ(7/2) = (5/2)·(3/2)·(1/2)√π = (15√π)/8,
  Γ(5/2) = (3/2)·(1/2)√π = (3√π)/4,
  Γ(6) = 5! = 120.

Thus,
  Γ(7/2) Γ(5/2) = (15√π/8) (3√π/4) = (45π)/32,
so that
  I₁ = 32 · (45π/32) / 120 = (45π)/120 = (3π)/8.

For I₂ we similarly get:
  I₂ = ∫₀² x^(3/2) (2–x)^(1/2) dx.
Under the substitution x = 2u, dx = 2 du, and 2–x = 2(1–u), we have:
  I₂ = ∫₀¹ (2u)^(3/2) [2(1–u)]^(1/2) (2 du)
    = 2^(3/2) u^(3/2) · 2^(1/2)(1–u)^(1/2) · 2 du
    = 2^(3/2+1/2+1) ∫₀¹ u^(3/2)(1–u)^(1/2) du
    = 2^(3+1) ∫₀¹ u^(3/2)(1–u)^(1/2) du  (note: 3/2+1/2 = 2)
    = 2³ ∫₀¹ u^(3/2)(1–u)^(1/2) du
    = 8 ∫₀¹ u^(3/2)(1–u)^(1/2) du.

Now write u^(3/2) = u^((5/2)–1) and (1–u)^(1/2) = (1–u)^((3/2)–1); hence a = 5/2, b = 3/2. Then:
  I₂ = 8 B(5/2, 3/2) = 8 · (Γ(5/2)Γ(3/2))/Γ(4).

We have already Γ(5/2) = (3√π)/4 and also
  Γ(3/2) = (1/2)√π,
and
  Γ(4) = 3! = 6.

Thus,
  Γ(5/2)Γ(3/2) = (3√π/4)(√π/2) = (3π)/8,
so that
  I₂ = 8 · (3π/8) / 6 = (3π)/6 = π/2.

Step 2. Now substitute I₁ and I₂ into the original expression:
  I = 8 I₁ – 12 I₂
   = 8 · (3π/8) – 12 · (π/2)
   = 3π – 6π
   = –3π.

Step 3. The numerical approximation is computed using π ≈ 3.141592653589793;
  –3π ≈ –3 × 3.141592653589793 ≈ –9.4247779608.

Thus, the final answer is:

{"answer": "$-3\\pi$", "numerical_answer": "$-9.4247779608$"}