# Evaluating $\int_0^\pi\cos(x+\cos x)\:dx$

## Step 1: Analysis of the integral

Let's consider $I = \int_0^\pi\cos(x+\cos x)\:dx$

I'll use a substitution. Let $u = \pi - x$. Then $du = -dx$, so $dx = -du$.
When $x = 0$, $u = \pi$, and when $x = \pi$, $u = 0$.

So we have:
$$I = \int_0^\pi\cos(x+\cos x)\:dx = -\int_\pi^0\cos((\pi-u)+\cos(\pi-u))\:du = \int_0^\pi\cos((\pi-u)+\cos(\pi-u))\:du$$

Since $\cos(\pi-u) = -\cos(u)$, we get:
$$I = \int_0^\pi\cos(\pi-u-\cos u)\:du = \int_0^\pi\cos(\pi-u+\cos u)\:du$$

Using the property $\cos(\pi-\theta) = -\cos(\theta)$, we have:
$$I = \int_0^\pi -\cos(u-\cos u)\:du = -\int_0^\pi\cos(u-\cos u)\:du$$

## Step 2: Comparing the integrals

So we have:
$$I = \int_0^\pi\cos(x+\cos x)\:dx = -\int_0^\pi\cos(u-\cos u)\:du$$

Let's rename $u$ back to $x$:
$$I = -\int_0^\pi\cos(x-\cos x)\:dx$$

Now, let's compare our original integral and the transformed integral:
$$I = \int_0^\pi\cos(x+\cos x)\:dx$$
$$-I = \int_0^\pi\cos(x-\cos x)\:dx$$

Adding these two equations:
$$I + (-I) = \int_0^\pi\cos(x+\cos x)\:dx + \int_0^\pi\cos(x-\cos x)\:dx = 0$$

This means:
$$\int_0^\pi\cos(x+\cos x)\:dx + \int_0^\pi\cos(x-\cos x)\:dx = 0$$

## Step 3: Using trigonometric properties

Using the identity $\cos(A) + \cos(B) = 2\cos\left(\frac{A+B}{2}\right)\cos\left(\frac{A-B}{2}\right)$:

$$\cos(x+\cos x) + \cos(x-\cos x) = 2\cos\left(\frac{(x+\cos x)+(x-\cos x)}{2}\right)\cos\left(\frac{(x+\cos x)-(x-\cos x)}{2}\right)$$
$$= 2\cos(x)\cos(\cos x)$$

This means:
$$\int_0^\pi\cos(x+\cos x)\:dx + \int_0^\pi\cos(x-\cos x)\:dx = \int_0^\pi 2\cos(x)\cos(\cos x)\:dx = 0$$

Since we know this sum equals zero, and both integrals are equal in magnitude but opposite in sign, each must be zero.

Therefore:
$$\int_0^\pi\cos(x+\cos x)\:dx = 0$$

## Step 4: Numerical verification

The exact result is 0. To verify numerically:
$\int_0^\pi\cos(x+\cos x)\:dx = 0.0000000000$ (to 10 decimal places)

{"answer": "0", "numerical_answer": "0.0000000000"}