We wish to evaluate

  I = ∫₋∞^∞ e^(–2x² – 5x – 3) dx.

Step 1. Complete the square in the exponent

Write the exponent as:
  –2x² – 5x – 3 = –2(x² + (5/2)x) – 3.

Complete the square for x² + (5/2)x:
  x² + (5/2)x = (x + 5/4)² – (5/4)² = (x + 5/4)² – 25/16.

Thus, the exponent becomes:
  –2[(x + 5/4)² – 25/16] – 3 = –2(x + 5/4)² + (50/16) – 3
               = –2(x + 5/4)² + (25/8) – 3.

Since 3 = 24/8, we have:
  (25/8 – 24/8) = 1/8.

So the exponent now is:
  –2(x + 5/4)² + 1/8,
and the integral becomes:
  I = e^(1/8) ∫₋∞^∞ e^(–2(x + 5/4)²) dx.

Step 2. Change of variables

Let u = x + 5/4 so that du = dx. The limits remain –∞ to ∞, and the integral becomes:
  I = e^(1/8) ∫₋∞^∞ e^(–2u²) du.

Step 3. Evaluate the Gaussian integral

Recall the standard result:
  ∫₋∞^∞ e^(–a u²) du = √(π/a),  for a > 0.

Here, a = 2, so:
  ∫₋∞^∞ e^(–2u²) du = √(π/2).

Thus, the exact value is:
  I = e^(1/8) √(π/2).

Step 4. Numerical approximation

We have:
  √(π/2) ≈ 1.2533141373  and  e^(1/8) ≈ 1.1331484531.
Multiplying these:
  I ≈ 1.1331484531 × 1.2533141373 ≈ 1.4204801580.

Final answer in the required JSON format:

{"answer": "\\sqrt{\\frac{\\pi}{2}}e^{\\frac{1}{8}}", "numerical_answer": "1.4204801580"}