To solve the definite integral \(\int_{0}^{2} x^{-1/2} (2-x)^{-1/2} [1-0.5x(2-x)]^{1} \, dx\), we will follow the steps outlined:

### Step 1: Simplify the integrand
First, let's simplify the integrand:
\[ f(x) = x^{-1/2} (2-x)^{-1/2} [1 - 0.5x(2-x)] \]

Notice that \(1 - 0.5x(2-x)\) can be simplified:
\[ 1 - 0.5x(2-x) = 1 - x + 0.5x^2 \]

Thus, the integrand becomes:
\[ f(x) = x^{-1/2} (2-x)^{-1/2} (1 - x + 0.5x^2) \]

### Step 2: Recognize the form of the integrand
The integrand \(x^{-1/2} (2-x)^{-1/2}\) suggests a form related to the Beta function. The Beta function \(B(a, b)\) is defined as:
\[ B(a, b) = \int_{0}^{1} t^{a-1} (1-t)^{b-1} \, dt \]

However, our limits of integration are from 0 to 2, not 0 to 1. We need to make a substitution to transform the integral into a form that matches the Beta function.

### Step 3: Substitution
Let \( t = \frac{x}{2} \). Then \( x = 2t \) and \( dx = 2 \, dt \). The limits of integration change from \( x = 0 \) to \( x = 2 \) to \( t = 0 \) to \( t = 1 \).

Substitute \( x = 2t \) into the integrand:
\[ f(2t) = (2t)^{-1/2} (2 - 2t)^{-1/2} [1 - 0.5(2t)(2 - 2t)] \]

Simplify each term:
\[ (2t)^{-1/2} = 2^{-1/2} t^{-1/2} \]
\[ (2 - 2t)^{-1/2} = 2^{-1/2} (1 - t)^{-1/2} \]
\[ 1 - 0.5(2t)(2 - 2t) = 1 - 2t + 2t^2 \]

Thus, the integrand becomes:
\[ f(2t) = 2^{-1/2} t^{-1/2} \cdot 2^{-1/2} (1 - t)^{-1/2} (1 - 2t + 2t^2) \]
\[ f(2t) = 2^{-1} t^{-1/2} (1 - t)^{-1/2} (1 - 2t + 2t^2) \]

Now, the integral becomes:
\[ \int_{0}^{2} f(x) \, dx = 2 \int_{0}^{1} 2^{-1} t^{-1/2} (1 - t)^{-1/2} (1 - 2t + 2t^2) \, dt \]
\[ = \int_{0}^{1} t^{-1/2} (1 - t)^{-1/2} (1 - 2t + 2t^2) \, dt \]

### Step 4: Recognize the Beta function form
The integral now resembles the Beta function form:
\[ \int_{0}^{1} t^{a-1} (1 - t)^{b-1} \, dt = B(a, b) \]

However, the additional polynomial term \(1 - 2t + 2t^2\) complicates direct application of the Beta function. We need to expand and integrate term by term.

### Step 5: Expand and integrate term by term
Expand the polynomial:
\[ 1 - 2t + 2t^2 \]

Thus, the integral becomes:
\[ \int_{0}^{1} t^{-1/2} (1 - t)^{-1/2} (1 - 2t + 2t^2) \, dt \]
\[ = \int_{0}^{1} t^{-1/2} (1 - t)^{-1/2} \, dt - 2 \int_{0}^{1} t^{1/2} (1 - t)^{-1/2} \, dt + 2 \int_{0}^{1} t^{3/2} (1 - t)^{-1/2} \, dt \]

Each of these integrals is a Beta function:
\[ \int_{0}^{1} t^{a-1} (1 - t)^{b-1} \, dt = B(a, b) \]

Thus:
\[ \int_{0}^{1} t^{-1/2} (1 - t)^{-1/2} \, dt = B\left(\frac{1}{2}, \frac{1}{2}\right) \]
\[ \int_{0}^{1} t^{1/2} (1 - t)^{-1/2} \, dt = B\left(\frac{3}{2}, \frac{1}{2}\right) \]
\[ \int_{0}^{1} t^{3/2} (1 - t)^{-1/2} \, dt = B\left(\frac{5}{2}, \frac{1}{2}\right) \]

Using the Beta function properties:
\[ B\left(\frac{1}{2}, \frac{1}{2}\right) = \pi \]
\[ B\left(\frac{3}{2}, \frac{1}{2}\right) = \frac{\Gamma\left(\frac{3}{2}\right) \Gamma\left(\frac{1}{2}\right)}{\Gamma(2)} = \frac{\frac{\sqrt{\pi}}{2} \sqrt{\pi}}{1} = \frac{\pi}{2} \]
\[ B\left(\frac{5}{2}, \frac{1}{2}\right) = \frac{\Gamma\left(\frac{5}{2}\right) \Gamma\left(\frac{1}{2}\right)}{\Gamma(3)} = \frac{\frac{3\sqrt{\pi}}{4} \sqrt{\pi}}{2} = \frac{3\pi}{8} \]

Thus, the integral becomes:
\[ \pi - 2 \cdot \frac{\pi}{2} + 2 \cdot \frac{3\pi}{8} \]
\[ = \pi - \pi + \frac{3\pi}{4} \]
\[ = \frac{3\pi}{4} \]

### Step 6: Numerical approximation
The numerical approximation of \(\frac{3\pi}{4}\) is:
\[ \frac{3\pi}{4} \approx 2.3561944901923448 \]

### Final Answer
\[
\boxed{
\begin{aligned}
\text{"answer": "}\frac{3\pi}{4}\text{"}, \\
\text{"numerical_answer": "2.3561944902"}
\end{aligned}
}
\]