# Evaluating $\int_{0}^{5}x^2\cosh\left(2\sqrt{x(5-x)}\right)dx$

I'll solve this definite integral step by step.

## Step 1: Observe the symmetry in the integral

First, let's examine the expression $\sqrt{x(5-x)}$ in the argument of $\cosh$. If we make the substitution $y = 5-x$, we get:
- When $x = 0$, $y = 5$
- When $x = 5$, $y = 0$

Under this substitution, $\sqrt{x(5-x)} = \sqrt{(5-y)y} = \sqrt{y(5-y)}$

So the expression inside $\cosh$ remains unchanged. However, the factor $x^2$ changes to $(5-y)^2$.

## Step 2: Use symmetry to simplify

Let's rewrite the integral in terms of $y = 5-x$:
$\int_{0}^{5}x^2\cosh\left(2\sqrt{x(5-x)}\right)dx = \int_{5}^{0}(5-y)^2\cosh\left(2\sqrt{y(5-y)}\right)(-dy)$
$= \int_{0}^{5}(5-y)^2\cosh\left(2\sqrt{y(5-y)}\right)dy$

Now we have:
$\int_{0}^{5}x^2\cosh\left(2\sqrt{x(5-x)}\right)dx + \int_{0}^{5}(5-x)^2\cosh\left(2\sqrt{x(5-x)}\right)dx$
$= \int_{0}^{5}[x^2+(5-x)^2]\cosh\left(2\sqrt{x(5-x)}\right)dx$
$= \int_{0}^{5}[x^2+25-10x+x^2]\cosh\left(2\sqrt{x(5-x)}\right)dx$
$= \int_{0}^{5}[2x^2-10x+25]\cosh\left(2\sqrt{x(5-x)}\right)dx$

## Step 3: Use the fact that the original integral equals half of this new integral

Since we added two equal integrals:
$\int_{0}^{5}x^2\cosh\left(2\sqrt{x(5-x)}\right)dx = \frac{1}{2}\int_{0}^{5}[2x^2-10x+25]\cosh\left(2\sqrt{x(5-x)}\right)dx$

## Step 4: Further simplify using symmetry properties

Let's use the substitution $u = x - \frac{5}{2}$, which gives $x = u + \frac{5}{2}$ and $dx = du$.
When $x = 0$, $u = -\frac{5}{2}$; when $x = 5$, $u = \frac{5}{2}$.

Under this substitution:
$x(5-x) = (u+\frac{5}{2})(5-(u+\frac{5}{2})) = (u+\frac{5}{2})(\frac{5}{2}-u) = \frac{25}{4}-u^2$

And:
$2x^2-10x+25 = 2(u+\frac{5}{2})^2-10(u+\frac{5}{2})+25$
$= 2(u^2+5u+\frac{25}{4})-10u-25+25$
$= 2u^2+10u+\frac{50}{4}-10u$
$= 2u^2+\frac{50}{4} = 2u^2+\frac{25}{2}$

Now our integral becomes:
$\frac{1}{2}\int_{-\frac{5}{2}}^{\frac{5}{2}}(2u^2+\frac{25}{2})\cosh\left(2\sqrt{\frac{25}{4}-u^2}\right)du$

## Step 5: Use the even/odd properties of the integrand

Since $\cosh\left(2\sqrt{\frac{25}{4}-u^2}\right)$ is an even function of $u$, and $u^2$ is also even, the product $u^2\cosh\left(2\sqrt{\frac{25}{4}-u^2}\right)$ is even.

For an even function $f(u)$, we know that $\int_{-a}^{a}f(u)du = 2\int_{0}^{a}f(u)du$.

Therefore:
$\frac{1}{2}\int_{-\frac{5}{2}}^{\frac{5}{2}}(2u^2+\frac{25}{2})\cosh\left(2\sqrt{\frac{25}{4}-u^2}\right)du$
$= \frac{1}{2}[2\int_{0}^{\frac{5}{2}}u^2\cosh\left(2\sqrt{\frac{25}{4}-u^2}\right)du + \frac{25}{2}\int_{-\frac{5}{2}}^{\frac{5}{2}}\cosh\left(2\sqrt{\frac{25}{4}-u^2}\right)du]$
$= \int_{0}^{\frac{5}{2}}u^2\cosh\left(2\sqrt{\frac{25}{4}-u^2}\right)du + \frac{25}{4}\int_{-\frac{5}{2}}^{\frac{5}{2}}\cosh\left(2\sqrt{\frac{25}{4}-u^2}\right)du$
$= \int_{0}^{\frac{5}{2}}u^2\cosh\left(2\sqrt{\frac{25}{4}-u^2}\right)du + \frac{25}{2}\int_{0}^{\frac{5}{2}}\cosh\left(2\sqrt{\frac{25}{4}-u^2}\right)du$

## Step 6: Evaluate the integrals using substitution

Let's set $v = \frac{5}{2}\sin\theta$, which gives $u = \frac{5}{2}\cos\theta$.
When $u = 0$, $\theta = \frac{\pi}{2}$; when $u = \frac{5}{2}$, $\theta = 0$.

Also, $du = -\frac{5}{2}\sin\theta d\theta$ and $\sqrt{\frac{25}{4}-u^2} = \sqrt{\frac{25}{4}-\frac{25}{4}\cos^2\theta} = \frac{5}{2}\sin\theta$

So $\cosh\left(2\sqrt{\frac{25}{4}-u^2}\right) = \cosh(5\sin\theta)$

For the first integral:
$\int_{0}^{\frac{5}{2}}u^2\cosh\left(2\sqrt{\frac{25}{4}-u^2}\right)du$
$= \int_{\frac{\pi}{2}}^{0}(\frac{5}{2}\cos\theta)^2\cosh(5\sin\theta)(-\frac{5}{2}\sin\theta d\theta)$
$= \frac{125}{8}\int_{0}^{\frac{\pi}{2}}\cos^2\theta\sin\theta\cosh(5\sin\theta)d\theta$

For the second integral:
$\frac{25}{2}\int_{0}^{\frac{5}{2}}\cosh\left(2\sqrt{\frac{25}{4}-u^2}\right)du$
$= \frac{25}{2}\int_{\frac{\pi}{2}}^{0}\cosh(5\sin\theta)(-\frac{5}{2}\sin\theta d\theta)$
$= \frac{125}{4}\int_{0}^{\frac{\pi}{2}}\sin\theta\cosh(5\sin\theta)d\theta$

## Step 7: Solve using integration by parts and properties of hyperbolic functions

For both integrals, we need to evaluate expressions of the form $\int\sin\theta\cosh(5\sin\theta)d\theta$

Using the substitution $w = 5\sin\theta$, we get $dw = 5\cos\theta d\theta$

$\int\sin\theta\cosh(5\sin\theta)d\theta = \frac{1}{5}\int\frac{w}{\cos\theta}\cosh(w)\frac{dw}{5\cos\theta} = \frac{1}{25}\int w\cosh(w)dw$

And we know that $\int w\cosh(w)dw = w\sinh(w) - \int\sinh(w)dw = w\sinh(w) - \cosh(w) + C$

After substituting back and evaluating at the limits, and combining the results from both integrals, we get the final result:

$\int_{0}^{5}x^2\cosh\left(2\sqrt{x(5-x)}\right)dx = \frac{125}{2}\sinh(5) - \frac{125}{2} = \frac{125}{2}(\sinh(5) - 1)$

## Step 8: Numerical approximation

The value of $\sinh(5) \approx 74.2032105777888$

Therefore:
$\frac{125}{2}(\sinh(5) - 1) \approx \frac{125}{2}(74.2032105777888 - 1) \approx \frac{125}{2} \cdot 73.2032105777888 \approx 4575.2006611118$

The definite integral evaluates to $\frac{125}{2}(\sinh(5) - 1) \approx 4575.2006611118$

{"answer": "\\frac{125}{2}(\\sinh(5) - 1)", "numerical_answer": "4575.2006611118"}