

To solve the definite integral \(\int_0^2 \frac{\arctan\left(\sqrt{x(2-x)}\right)}{x(2-x)} \, dx\), we proceed with the following steps:

### Step 1: Simplify the integrand using substitution
First, observe that \(x(2-x) = 1 - (x-1)^2\) (by completing the square). Let \(x = 1 + \sin\theta\), so \(dx = \cos\theta \, d\theta\). The limits of integration transform as follows: when \(x=0\), \(\theta = -\pi/2\); when \(x=2\), \(\theta = \pi/2\). Substituting, we get:
\[
\sqrt{x(2-x)} = \sqrt{1 - \sin^2\theta} = \cos\theta \quad (\text{since } \cos\theta \geq 0 \text{ for } \theta \in [-\pi/2, \pi/2]).
\]
The integrand becomes:
\[
\frac{\arctan(\cos\theta)}{(1+\sin\theta)(1-\sin\theta)} \cdot \cos\theta \, d\theta = \frac{\arctan(\cos\theta)}{\cos^2\theta} \cdot \cos\theta \, d\theta = \frac{\arctan(\cos\theta)}{\cos\theta} \, d\theta.
\]
The integral simplifies to:
\[
\int_{-\pi/2}^{\pi/2} \frac{\arctan(\cos\theta)}{\cos\theta} \, d\theta.
\]
Since the integrand is even, this becomes:
\[
2 \int_0^{\pi/2} \frac{\arctan(\cos\theta)}{\cos\theta} \, d\theta.
\]

### Step 2: Use differentiation under the integral sign
Let \(I(t) = \int_0^{\pi/2} \frac{\arctan(t \sin\phi)}{\sin\phi} \, d\phi\). We aim to relate our integral to \(I(t)\). By symmetry, \(\int_0^{\pi/2} \frac{\arctan(\cos\theta)}{\cos\theta} \, d\theta = \int_0^{\pi/2} \frac{\arctan(\sin\phi)}{\sin\phi} \, d\phi\) (using \(\phi = \pi/2 - \theta\)), so our integral is \(2I(1)\).

Differentiate \(I(t)\) with respect to \(t\):
\[
I'(t) = \int_0^{\pi/2} \frac{1}{1 + t^2 \sin^2\phi} \, d\phi.
\]
Using the substitution \(u = \tan\phi\) (so \(du = \sec^2\phi \, d\phi\)), the integral becomes:
\[
I'(t) = \int_0^\infty \frac{1}{1 + t^2 \cdot \frac{u^2}{1 + u^2}} \cdot \frac{du}{1 + u^2} = \int_0^\infty \frac{1}{1 + u^2 + t^2 u^2} \, du = \int_0^\infty \frac{1}{1 + u^2(1 + t^2)} \, du.
\]
This evaluates to:
\[
I'(t) = \frac{\pi}{2\sqrt{1 + t^2}}.
\]

### Step 3: Integrate \(I'(t)\) to find \(I(t)\)
Integrate \(I'(t)\) with respect to \(t\):
\[
I(t) = \frac{\pi}{2} \int \frac{1}{\sqrt{1 + t^2}} \, dt = \frac{\pi}{2} \ln\left(t + \sqrt{1 + t^2}\right) + C.
\]
Using \(I(0) = 0\) (since \(\arctan(0) = 0\)), we find \(C = 0\). Thus:
\[
I(t) = \frac{\pi}{2} \ln\left(t + \sqrt{1 + t^2}\right).
\]

### Step 4: Evaluate the original integral
Our integral is \(2I(1)\):
\[
2I(1) = 2 \cdot \frac{\pi}{2} \ln\left(1 + \sqrt{1 + 1}\right) = \pi \ln\left(1 + \sqrt{2}\right).
\]

### Numerical Approximation
The numerical value of \(\pi \ln(1 + \sqrt{2})\) is approximately \(2.7680630452\).

{"answer": "\(\pi \ln\left(1 + \sqrt{2}\right)\)", "numerical_answer": "2.7680630452"}