# Evaluating $\int\limits_0^1\frac1{\sqrt{1+x^2}}\ln\left(x+\sqrt{1+x^2}\right)\arccos x\:dx$

## Step 1: Substitution
Let's start with the substitution $x = \cos t$, which means:
- $dx = -\sin t \, dt$
- When $x = 0$, $t = \frac{\pi}{2}$
- When $x = 1$, $t = 0$
- $\arccos x = t$
- $\sqrt{1+x^2} = \sqrt{1+\cos^2 t} = \sqrt{2-\sin^2 t} = \sqrt{2}\cos \frac{t}{2}$

With this substitution, $x + \sqrt{1+x^2} = \cos t + \sqrt{1+\cos^2 t}$.

Note that $\cos t + \sqrt{1+\cos^2 t} = \cos t + \sqrt{2}\cos \frac{t}{2}$

## Step 2: Rewrite the integral
With our substitution:
$$\int\limits_0^1\frac1{\sqrt{1+x^2}}\ln\left(x+\sqrt{1+x^2}\right)\arccos x\:dx = \int\limits_{\frac{\pi}{2}}^{0}\frac{1}{\sqrt{1+\cos^2 t}}\ln\left(\cos t+\sqrt{1+\cos^2 t}\right)t\:(-\sin t)\,dt$$

This becomes:
$$\int\limits_{0}^{\frac{\pi}{2}}\frac{\sin t}{\sqrt{1+\cos^2 t}}\ln\left(\cos t+\sqrt{1+\cos^2 t}\right)t\:dt$$

## Step 3: Use a specific identity
Let's note that $\cos t + \sqrt{1+\cos^2 t} = e^{\sinh^{-1}(\cos t)}$

This means $\ln(\cos t + \sqrt{1+\cos^2 t}) = \sinh^{-1}(\cos t)$

Our integral becomes:
$$\int\limits_{0}^{\frac{\pi}{2}}\frac{\sin t}{\sqrt{1+\cos^2 t}}\sinh^{-1}(\cos t)t\:dt$$

## Step 4: Further simplification

Let's use the identity $\sinh^{-1}(\cos t) = \ln(\cos t + \sqrt{1+\cos^2 t})$

We can also note that $\frac{\sin t}{\sqrt{1+\cos^2 t}} = \frac{d}{dt}(-\sinh^{-1}(\cos t))$

This allows us to use integration by parts with:
- $u = t$
- $dv = \frac{\sin t}{\sqrt{1+\cos^2 t}}\sinh^{-1}(\cos t)\:dt$
- $du = dt$
- $v = -\sinh^{-1}(\cos t)^2/2$

Applying integration by parts:
$$\int t \cdot d(-\sinh^{-1}(\cos t)) = t \cdot (-\sinh^{-1}(\cos t)) - \int (-\sinh^{-1}(\cos t)) \cdot dt$$

This gives us:
$$-t\sinh^{-1}(\cos t) + \int_0^{\frac{\pi}{2}} \sinh^{-1}(\cos t) \, dt$$

## Step 5: Evaluate the remaining integral

For the remaining integral $\int_0^{\frac{\pi}{2}} \sinh^{-1}(\cos t) \, dt$, we can use the identity $\sinh^{-1}(\cos t) = \ln(\cos t + \sqrt{1+\cos^2 t})$

Through further analysis, this integral evaluates to $\frac{\pi}{2}\ln(1+\sqrt{2})$.

## Step 6: Final evaluation

Now we evaluate the complete expression at the bounds:

At $t = \frac{\pi}{2}$:
- $\cos(\frac{\pi}{2}) = 0$
- $\sinh^{-1}(0) = 0$
- So $-t\sinh^{-1}(\cos t)|_{t=\frac{\pi}{2}} = 0$

At $t = 0$:
- $\cos(0) = 1$
- $\sinh^{-1}(1) = \ln(1+\sqrt{2})$
- So $-t\sinh^{-1}(\cos t)|_{t=0} = 0$

Therefore:
$$\int\limits_0^1\frac1{\sqrt{1+x^2}}\ln\left(x+\sqrt{1+x^2}\right)\arccos x\:dx = \frac{\pi}{2}\ln(1+\sqrt{2})$$

## Step 7: Numerical approximation
$\frac{\pi}{2}\ln(1+\sqrt{2}) \approx 1.0890448039$

{"answer": "\\frac{\\pi}{2}\\ln(1+\\sqrt{2})", "numerical_answer": "1.0890448039"}