<think>
Okay, so I need to compute the definite integral of cos(x + cos(x)) from 0 to π. Hmm, let's start by thinking about how to approach this. The integral is ∫₀^π cos(x + cos(x)) dx. 

First, I remember that integrating functions with compositions like cos(x + cos(x)) can be tricky. Maybe there's a substitution or some symmetry I can use here. Let me check if the integrand has any symmetry over the interval [0, π]. 

The function inside the cosine is x + cos(x). Let's see, when x is replaced by π - x, what happens? Let's substitute x with π - t. If I let t = π - x, then when x = 0, t = π, and when x = π, t = 0. The differential dx becomes -dt. So the integral becomes ∫ from π to 0 of cos(π - t + cos(π - t)) (-dt) which is the same as ∫₀^π cos(π - t + cos(π - t)) dt. 

Now, cos(π - t) is equal to -cos(t), right? Because cosine is an even function and cos(π - t) = -cos(t). So substituting that in, the argument becomes π - t + (-cos(t)) = π - t - cos(t). So the integral becomes ∫₀^π cos(π - t - cos(t)) dt. 

But cos(π - a) is equal to -cos(a), so cos(π - t - cos(t)) = cos(π - (t + cos(t))) = -cos(t + cos(t)). Wait, the integral now is ∫₀^π -cos(t + cos(t)) dt. But the original integral is ∫₀^π cos(x + cos(x)) dx. So if I add these two expressions together, the original integral I and the transformed one would be I = ∫₀^π cos(x + cos(x)) dx and the transformed integral is -I. So adding them: I + (-I) = 0. But wait, that can't be right. Wait, maybe I made a mistake here.

Wait, let me clarify. Let me denote the original integral as I. After substitution, we have I = ∫₀^π cos(x + cos(x)) dx. Then, substituting x = π - t, we get I = ∫₀^π cos(π - t + cos(π - t)) dt. As cos(π - t) = -cos(t), so the argument becomes π - t - cos(t). Then, cos(π - t - cos(t)) = cos(π - (t + cos(t))) = -cos(t + cos(t)) because cos(π - θ) = -cosθ. Therefore, the integral becomes ∫₀^π -cos(t + cos(t)) dt = -I. So we have I = -I, which implies that 2I = 0, so I = 0. 

Wait, that's interesting. So according to this substitution, the integral from 0 to π of cos(x + cos(x)) dx is equal to its negative, which would mean the integral is zero. Is that possible? Let me check with a numerical approximation to see if that's the case. 

But before that, let me verify the substitution steps again. The substitution x = π - t, dx = -dt. The limits go from π to 0, which flips back to 0 to π with a negative sign. Then, the integrand becomes cos(π - t + cos(π - t)) = cos(π - t - cos(t)) because cos(π - t) is -cos(t). Then, using the identity cos(π - a) = -cos(a), so cos(π - t - cos(t)) = cos(π - (t + cos(t))) = -cos(t + cos(t)). Therefore, the integral becomes ∫₀^π -cos(t + cos(t)) dt = -I. Therefore, I = -I, so 2I = 0, hence I = 0. 

So analytically, the integral is zero. Let me check this with a numerical approximation. Let's compute the integral numerically. For example, using a calculator or some estimation. Let's approximate the integral ∫₀^π cos(x + cos(x)) dx. 

Alternatively, maybe I can use a series expansion or some other method. But if the analytical result is zero, the numerical approximation should be very close to zero. Let me try to compute it numerically. 

Alternatively, maybe there's a mistake in the substitution. Let me check again. Suppose f(x) = cos(x + cos(x)). Then, f(π - x) = cos(π - x + cos(π - x)) = cos(π - x - cos(x)) = cos(π - (x + cos(x))) = -cos(x + cos(x)). Therefore, f(π - x) = -f(x). Therefore, the function is odd with respect to the midpoint of the interval [0, π], which is π/2. Therefore, integrating from 0 to π, the integral of an odd function around π/2 would be zero. 

Yes, that makes sense. Because if we make the substitution u = π/2 - t, but perhaps the key is that the function is symmetric in such a way that the positive and negative areas cancel out. Therefore, the exact value of the integral is zero, and the numerical approximation should be very close to zero. 

To confirm, let's compute the integral numerically. Let's split the integral into parts. For example, from 0 to π/2 and π/2 to π. Let's compute each part. 

Alternatively, use numerical methods like Simpson's rule or use a calculator. Let's approximate the integral from 0 to π of cos(x + cos(x)) dx. 

But since I can't compute it here exactly, but if the analytical result is zero, the numerical approximation should be very small. Let me check with a simple approximation. Let's approximate the integral using the trapezoidal rule with a few intervals. 

Take n = 4 intervals. The interval from 0 to π is divided into 4 parts: 0, π/4, π/2, 3π/4, π. Compute the function at these points:

At x=0: cos(0 + cos(0)) = cos(0 + 1) = cos(1) ≈ 0.54030230586

At x=π/4: cos(π/4 + cos(π/4)) ≈ cos(π/4 + √2/2) ≈ cos(0.7854 + 0.7071) ≈ cos(1.4925) ≈ 0.07703

At x=π/2: cos(π/2 + cos(π/2)) = cos(π/2 + 0) = cos(π/2) = 0

At x=3π/4: cos(3π/4 + cos(3π/4)) ≈ cos(3π/4 - √2/2) ≈ cos(2.3562 - 0.7071) ≈ cos(1.6491) ≈ -0.07703

At x=π: cos(π + cos(π)) = cos(π + (-1)) = cos(π -1) ≈ cos(2.1416) ≈ -0.54030230586

Now, applying the trapezoidal rule:

Δx = π/4 ≈ 0.7854

Integral ≈ Δx/2 [f(0) + 2f(π/4) + 2f(π/2) + 2f(3π/4) + f(π)]

= (0.7854/2) [0.5403 + 2*0.07703 + 2*0 + 2*(-0.07703) + (-0.5403)]

Calculate the terms inside:

0.5403 + 2*0.07703 = 0.5403 + 0.15406 = 0.69436

Then, 2*0 = 0

Then, 2*(-0.07703) = -0.15406

Then, -0.5403

So total inside: 0.69436 + 0 -0.15406 -0.5403 = 0.69436 -0.15406 = 0.5403; 0.5403 -0.5403 = 0

So the trapezoidal estimate with 4 intervals gives 0.7854/2 * 0 = 0. So that's zero. But this is a very rough approximation. Let's try with more intervals. Maybe take n=2 intervals. Wait, but even with n=4, it's zero. That's interesting. Let's try with n=6 or something. Wait, but maybe the function is odd around π/2, so the integral cancels out exactly. For example, if we take pairs of points symmetric around π/2, their contributions cancel. 

For example, x and π -x. For each x in [0, π/2], there's a corresponding point π -x in [π/2, π]. The function at x is cos(x + cos(x)), and at π -x is cos(π -x + cos(π -x)) = cos(π -x -cos(x)) = -cos(x + cos(x)). Therefore, the sum of f(x) + f(π -x) = cos(x + cos(x)) - cos(x + cos(x)) = 0. Therefore, when integrating from 0 to π, splitting the integral into [0, π/2] and [π/2, π], and substituting t = π -x in the second part, we get that the integral over [π/2, π] is the negative of the integral over [0, π/2]. Therefore, the total integral is zero. 

Therefore, the exact value is zero, and any numerical approximation should be very close to zero. 

But to confirm, let's compute a numerical approximation with higher precision. For example, using a calculator or computational tool. But since I can't do that here, I can reason that due to the symmetry, the integral is exactly zero. Therefore, the exact answer is 0, and the numerical approximation is 0.0000000000.
</think>

{"answer": "0", "numerical_answer": "0.0000000000"}