<think>
Okay, let's tackle this integral step by step. The integral given is from 0 to 2 of x^(-1/4) times (2 - x)^(-3/4) times cosh(1 times the fourth root of x(2 - x)) dx. Hmm, that looks a bit complicated, but maybe there's a substitution that can simplify it.

First, I notice that the exponents on x and (2 - x) are -1/4 and -3/4, which add up to -1. Also, the argument inside the cosh function is the fourth root of x(2 - x). Maybe a substitution involving the term inside the cosh would help. Let me think about substituting t = x(2 - x), but I need to check if that's useful. Alternatively, perhaps a substitution that combines x and (2 - x) in a way that simplifies the exponents. Let's try a substitution that can turn the product x(2 - x) into something squared or another manageable form.

Wait, another thought: the limits of integration are from 0 to 2. That's symmetric around x = 1. Maybe a substitution like u = x - 1 could center the integral around zero, but I'm not sure yet. Let's see. Alternatively, maybe a trigonometric substitution. Let me think: if I set x = 2 sin^2(theta), then 2 - x would be 2 cos^2(theta). Let's try that. Let’s let x = 2 sin^2θ. Then dx would be 4 sinθ cosθ dθ. Let's see what happens to the integral. Let's substitute:

x = 2 sin²θ, so when x=0, θ=0, and when x=2, θ=π/2. Then 2 - x = 2 cos²θ. The term x(2 - x) becomes 2 sin²θ * 2 cos²θ = 4 sin²θ cos²θ, so the fourth root of that would be sqrt(sinθ cosθ) * sqrt(2). Wait, the fourth root of 4 sin²θ cos²θ is (4 sin²θ cos²θ)^(1/4) = (4)^(1/4) * (sinθ cosθ)^(1/2) = sqrt(2) * sqrt(sinθ cosθ). But the argument inside cosh is 1 times that, so sqrt(2) * sqrt(sinθ cosθ). Hmm, not sure if that's helpful yet.

But let's proceed with substitution. The integral becomes:

∫ from θ=0 to θ=π/2 of [ (2 sin²θ)^(-1/4) * (2 cos²θ)^(-3/4) ) ] * cosh( sqrt(2) sqrt(sinθ cosθ) ) * 4 sinθ cosθ dθ.

Let's simplify the terms:

First, (2 sin²θ)^(-1/4) = 2^(-1/4) * sin^(-1/2)θ

Similarly, (2 cos²θ)^(-3/4) = 2^(-3/4) * cos^(-3/2)θ

Multiplying these together: 2^(-1/4 - 3/4) * sin^(-1/2)θ * cos^(-3/2)θ = 2^(-1) * sin^(-1/2)θ cos^(-3/2)θ = (1/2) * [1/(sin^(1/2)θ cos^(3/2)θ)]

Then, the rest of the integrand is cosh( sqrt(2) sqrt(sinθ cosθ) ) * 4 sinθ cosθ dθ.

Putting it all together:

(1/2) * [1/(sin^(1/2)θ cos^(3/2)θ)] * cosh( sqrt(2) sqrt(sinθ cosθ) ) * 4 sinθ cosθ dθ

Simplify the coefficients: 1/2 * 4 = 2

The terms with sin and cos:

[1/(sin^(1/2)θ cos^(3/2)θ)] * sinθ cosθ = sin^(1/2)θ * cos^(-1/2)θ

So the integral becomes:

2 ∫ sin^(1/2)θ cos^(-1/2)θ * cosh( sqrt(2) sqrt(sinθ cosθ) ) dθ from 0 to π/2.

Hmm, maybe another substitution here. Let me set t = sqrt(sinθ cosθ). But perhaps a substitution that can relate to the argument of the cosh function. Let's let u = sqrt(2) * sqrt(sinθ cosθ). Then u^2 = 2 sinθ cosθ = sin(2θ). Wait, because sin(2θ) = 2 sinθ cosθ. So u^2 = sin(2θ). Then, perhaps expressing in terms of u.

But maybe another approach. Let's note that sinθ cosθ = (1/2) sin(2θ). So sqrt(sinθ cosθ) = sqrt( (1/2) sin(2θ) ) = (1/√2) sqrt(sin(2θ)). Then the argument inside cosh becomes sqrt(2) * (1/√2) sqrt(sin(2θ)) ) = sqrt(sin(2θ)). So the cosh term is cosh( sqrt(sin(2θ)) ). Hmm, that might not immediately help, but let's proceed.

Alternatively, let's make a substitution for 2θ. Let’s set φ = 2θ. Then when θ=0, φ=0; θ=π/2, φ=π. Then dφ = 2 dθ, so dθ = dφ/2. Then the integral becomes:

2 ∫_{φ=0}^{φ=π} [ sin^(1/2)(φ/2) cos^(-1/2)(φ/2) ] * cosh( sqrt(sinφ) ) * (dφ/2)

Wait, the original substitution was θ = φ/2. So sinθ = sin(φ/2), cosθ = cos(φ/2). Then sinθ cosθ = sin(φ/2) cos(φ/2) = (1/2) sinφ. So sqrt(sinθ cosθ) = sqrt( (1/2) sinφ ) = (1/√2) sqrt(sinφ). Then the argument of cosh is sqrt(2) * (1/√2) sqrt(sinφ) ) = sqrt(sinφ). So the cosh term becomes cosh( sqrt(sinφ) ). 

So the integral becomes:

2 * (1/2) ∫_{0}^{π} [ sin^(1/2)(φ/2) cos^(-1/2)(φ/2) ] * cosh( sqrt(sinφ) ) dφ

Which is:

∫_{0}^{π} [ sin^(1/2)(φ/2) cos^(-1/2)(φ/2) ] * cosh( sqrt(sinφ) ) dφ

Hmm, not sure if that's better. Let's look at the term sin^(1/2)(φ/2) cos^(-1/2)(φ/2). That can be written as [ sin(φ/2) / cos(φ/2) ]^(1/2) = [ tan(φ/2) ]^(1/2). But I'm not sure if that helps. Alternatively, perhaps using the identity sin(φ/2) = sqrt( (1 - cosφ)/2 ), cos(φ/2) = sqrt( (1 + cosφ)/2 ). So sin(φ/2)/cos(φ/2) = sqrt( (1 - cosφ)/(1 + cosφ) ) = tan(φ/2). So maybe that's not helpful here.

Alternatively, perhaps another substitution. Let me consider t = sqrt(sinφ). Then t^2 = sinφ, so 2t dt = cosφ dφ. Wait, but that might complicate things. Let's see:

If t = sqrt(sinφ), then φ goes from 0 to π, so t goes from 0 to 1 and back to 0. Hmm, maybe not helpful. Alternatively, perhaps split the integral into two parts from 0 to π/2 and π/2 to π. But I'm not sure.

Alternatively, maybe consider a substitution that can turn the integral into a standard form. Let's recall that the integral involves cosh of sqrt(sinφ), which might relate to some known integral involving hypergeometric functions or Bessel functions. But I'm not sure. Alternatively, maybe expanding the cosh term as a Taylor series and integrating term by term.

Let me try that cosh(z) = sum_{n=0}^infty z^{2n}/(2n)! So, if we can express the integral as a sum, maybe we can integrate term by term.

So, let's write cosh( sqrt(sinφ) ) = sum_{n=0}^infty (sinφ)^n / (2n)! )

Then the integral becomes sum_{n=0}^infty [1/(2n)!] ∫_{0}^{π} [ sin^(1/2)(φ/2) cos^(-1/2)(φ/2) ] * sin^nφ dφ

But this seems complicated. Let me check if there's a better substitution.

Wait, going back to the original substitution. Let me think again. The original integral after substitution became:

2 ∫_{0}^{π/2} sin^(1/2)θ cos^(-1/2)θ * cosh( sqrt(sin(2θ)) ) dθ

Wait, because when we had x = 2 sin²θ, then x(2 - x) = 4 sin²θ cos²θ, so sqrt[ x(2 - x) ] = 2 sinθ cosθ = sin(2θ). Wait, no: sqrt[ x(2 - x) ] is sqrt(4 sin²θ cos²θ) = 2 sinθ cosθ = sin(2θ). But the original argument inside cosh is the fourth root, which is [x(2 - x)]^{1/4} = [4 sin²θ cos²θ]^{1/4} = (4)^{1/4} (sinθ cosθ)^{1/2} = sqrt(2) (sinθ cosθ)^{1/2} = sqrt(2) * sqrt(sinθ cosθ). But sinθ cosθ = (1/2) sin(2θ), so sqrt(sinθ cosθ) = sqrt( (1/2) sin(2θ) ) = (1/√2) sqrt(sin(2θ)). Therefore, the argument inside cosh is sqrt(2) * (1/√2) sqrt(sin(2θ)) ) = sqrt(sin(2θ)). So the integral becomes:

2 ∫_{0}^{π/2} sin^(1/2)θ cos^(-1/2)θ * cosh( sqrt(sin(2θ)) ) dθ

Hmm, maybe changing variable to t = 2θ. Let’s set t = 2θ, so θ = t/2, dθ = dt/2. When θ=0, t=0; θ=π/2, t=π. Then the integral becomes:

2 ∫_{0}^{π} [ sin^(1/2)(t/2) cos^(-1/2)(t/2) ] * cosh( sqrt(sin t) ) * (dt/2)

Which simplifies to:

∫_{0}^{π} [ sin^(1/2)(t/2) cos^(-1/2)(t/2) ] * cosh( sqrt(sin t) ) dt

Hmm, still not obvious. Let's look at the term sin^(1/2)(t/2) cos^(-1/2)(t/2). Let's express this as [ sin(t/2) / cos(t/2) ]^(1/2) = [ tan(t/2) ]^(1/2). Alternatively, using the identity, tan(t/2) = (1 - cos t)/sin t. Not sure. Alternatively, perhaps express in terms of sin t. Let's note that sin(t/2) = sqrt( (1 - cos t)/2 ), cos(t/2) = sqrt( (1 + cos t)/2 ). So sin(t/2)/cos(t/2) = sqrt( (1 - cos t)/(1 + cos t) ) = tan(t/2). So [ sin(t/2)/cos(t/2) ]^(1/2) = [ tan(t/2) ]^(1/2). Hmm, but integrating this with cosh(sqrt(sin t)) from 0 to π is still not straightforward.

Alternatively, maybe another substitution. Let’s consider u = sqrt(sin t). Then t goes from 0 to π, so u goes from 0 to 1 and back to 0. But integrating over u might not be helpful. Alternatively, split the integral into two parts: from 0 to π/2 and π/2 to π. Let’s try that.

Let’s split the integral into I = ∫_{0}^{π/2} ... dt + ∫_{π/2}^{π} ... dt. For the second integral, let’s make a substitution t = π - s. Then when t = π/2, s = π/2; t = π, s = 0. Then dt = -ds. The integral becomes:

∫_{π/2}^{π} [ sin^(1/2)(t/2) cos^(-1/2)(t/2) ] * cosh( sqrt(sin t) ) dt = ∫_{0}^{π/2} [ sin^(1/2)( (π - s)/2 ) cos^(-1/2)( (π - s)/2 ) ] * cosh( sqrt(sin(π - s)) ) ds

But sin(π - s) = sin s, and (π - s)/2 = π/2 - s/2. So sin( (π - s)/2 ) = sin(π/2 - s/2) = cos(s/2), and cos( (π - s)/2 ) = cos(π/2 - s/2) = sin(s/2). Therefore, the term becomes [ cos(s/2) / sin(s/2) ]^(1/2) = [ cot(s/2) ]^(1/2). So the second integral becomes:

∫_{0}^{π/2} [ cot(s/2) ]^(1/2) * cosh( sqrt(sin s) ) ds

But the original first integral is ∫_{0}^{π/2} [ tan(t/2) ]^(1/2) * cosh( sqrt(sin t) ) dt. So combining both parts, the total integral I becomes:

∫_{0}^{π/2} [ tan(t/2)^(1/2) + cot(t/2)^(1/2) ] * cosh( sqrt(sin t) ) dt

But tan(t/2) + cot(t/2) = [sin(t/2)/cos(t/2) + cos(t/2)/sin(t/2)] = [sin²(t/2) + cos²(t/2)] / [sin(t/2)cos(t/2)] = 1 / [sin(t/2)cos(t/2)] = 2 / sin t. But here we have the sum of square roots, not the sum of the terms themselves. So sqrt(tan(t/2)) + sqrt(cot(t/2)) = sqrt(sin(t/2)/cos(t/2)) + sqrt(cos(t/2)/sin(t/2)) = [sin(t/2) + cos(t/2)] / sqrt(sin(t/2)cos(t/2)). Let's compute that:

sqrt(tan(t/2)) + sqrt(cot(t/2)) = sqrt(sin(t/2)/cos(t/2)) + sqrt(cos(t/2)/sin(t/2)) = [sin(t/2) + cos(t/2)] / sqrt(sin(t/2)cos(t/2))

So the integral becomes:

∫_{0}^{π/2} [ (sin(t/2) + cos(t/2)) / sqrt(sin(t/2)cos(t/2)) ] * cosh( sqrt(sin t) ) dt

Let’s compute the denominator: sqrt(sin(t/2)cos(t/2)) = sqrt( (1/2) sin t ) by the identity sin t = 2 sin(t/2) cos(t/2). So sqrt(sin(t/2)cos(t/2)) = sqrt( (sin t)/2 ). Therefore, the denominator is sqrt(sin t / 2) = (sin t)^(1/2) / 2^(1/2). So the numerator is sin(t/2) + cos(t/2). Therefore, the entire expression becomes:

[ sin(t/2) + cos(t/2) ] / ( (sin t)^(1/2) / 2^(1/2) ) ) = 2^(1/2) [ sin(t/2) + cos(t/2) ] / (sin t)^(1/2)

So the integral is:

2^(1/2) ∫_{0}^{π/2} [ sin(t/2) + cos(t/2) ] / (sin t)^(1/2) * cosh( sqrt(sin t) ) dt

Hmm, maybe this is leading somewhere. Let's see if we can express [ sin(t/2) + cos(t/2) ] in terms of sqrt(sin t). Let's compute [ sin(t/2) + cos(t/2) ]^2 = sin²(t/2) + 2 sin(t/2)cos(t/2) + cos²(t/2) = 1 + sin t. Therefore, sin(t/2) + cos(t/2) = sqrt(1 + sin t). So substituting back:

2^(1/2) ∫_{0}^{π/2} sqrt(1 + sin t) / sqrt(sin t) * cosh( sqrt(sin t) ) dt

So this simplifies to:

2^(1/2) ∫_{0}^{π/2} sqrt( (1 + sin t)/sin t ) * cosh( sqrt(sin t) ) dt

But (1 + sin t)/sin t = 1/sin t + 1. Hmm, not sure. Alternatively, note that sqrt( (1 + sin t)/sin t ) = sqrt(1/sin t + 1). Alternatively, perhaps another substitution. Let’s set y = sqrt(sin t). Then y^2 = sin t, so 2y dy = cos t dt. But cos t = sqrt(1 - y^4), since sin t = y^2. Wait, cos t = sqrt(1 - sin²t) = sqrt(1 - y^4). So dt = 2y dy / sqrt(1 - y^4). Let's try this.

So when t goes from 0 to π/2, y goes from 0 to 1. The integral becomes:

2^(1/2) ∫_{0}^{1} sqrt( (1 + y^2)/y^2 ) * cosh(y) * (2y / sqrt(1 - y^4)) dy

Wait, let's check:

sqrt( (1 + sin t)/sin t ) = sqrt( (1 + y^2)/y^2 ) = sqrt(1/y^2 + 1) = sqrt( (1 + y^2)/y^2 ) = sqrt(1 + y^2)/y

So substituting:

2^(1/2) * ∫0^1 [ sqrt(1 + y^2)/y ] * cosh(y) * [ 2y / sqrt(1 - y^4) ] dy

Wait, wait, the substitution was dt = 2y dy / sqrt(1 - y^4). So the integral becomes:

2^(1/2) * ∫0^1 [ sqrt(1 + y^2)/y ] * cosh(y) * (2y dy / sqrt(1 - y^4)) )

Simplify terms:

sqrt(1 + y^2)/y * 2y = 2 sqrt(1 + y^2)

And the denominator sqrt(1 - y^4) remains. So:

2^(1/2) * 2 ∫0^1 [ sqrt(1 + y^2) / sqrt(1 - y^4) ] * cosh(y) dy

Which is 2^(3/2) ∫0^1 [ sqrt(1 + y^2) / sqrt(1 - y^4) ] * cosh(y) dy

But 1 - y^4 = (1 - y^2)(1 + y^2), so sqrt(1 - y^4) = sqrt(1 - y^2) sqrt(1 + y^2). Therefore:

sqrt(1 + y^2)/sqrt(1 - y^4) = sqrt(1 + y^2) / [ sqrt(1 - y^2) sqrt(1 + y^2) ) ] = 1 / sqrt(1 - y^2)

So the integral simplifies to:

2^(3/2) ∫0^1 [1 / sqrt(1 - y^2)] * cosh(y) dy

Ah! Now this is a much simpler integral. So the integral reduces to 2^(3/2) times the integral from 0 to 1 of cosh(y) / sqrt(1 - y^2) dy.

This is a standard integral. Let's recall that ∫ cosh(ay) / sqrt(1 - y^2) dy from 0 to 1 is related to the modified Bessel function of the first kind. Specifically, ∫0^1 cosh(ay) / sqrt(1 - y^2) dy = (π/2) I_0(a), where I_0 is the modified Bessel function. In our case, a = 1, so the integral becomes (π/2) I_0(1).

Therefore, the original integral is 2^(3/2) * (π/2) I_0(1) = 2^(1/2) π I_0(1) = sqrt(2) π I_0(1).

But wait, let me verify this. The integral ∫0^1 cosh(y)/sqrt(1 - y^2) dy. Let’s check substitution: set y = sinθ, then dy = cosθ dθ, and sqrt(1 - y^2) = cosθ. The integral becomes ∫0^{π/2} cosh(sinθ) dθ. Hmm, but I thought it relates to Bessel functions. Let me recall that the modified Bessel function of the first kind I_0(z) is given by (1/π) ∫0^π e^{z cosθ} dθ. Alternatively, there's an integral representation involving cosh(z sinθ). Let me check:

Yes, I_0(z) = (1/π) ∫0^π cosh(z sinθ) dθ. So if we set z = 1, then I_0(1) = (1/π) ∫0^π cosh(sinθ) dθ. But our integral is ∫0^{π/2} cosh(sinθ) dθ. Wait, but if we extend the integral to π, then:

∫0^{π} cosh(sinθ) dθ = 2 ∫0^{π/2} cosh(sinθ) dθ, because cosh(sinθ) is symmetric around θ = π/2. Therefore, I_0(1) = (1/π) * 2 ∫0^{π/2} cosh(sinθ) dθ. Therefore, ∫0^{π/2} cosh(sinθ) dθ = (π/2) I_0(1). But our substitution led to ∫0^1 cosh(y)/sqrt(1 - y^2) dy = ∫0^{π/2} cosh(sinθ) dθ = (π/2) I_0(1). Therefore, the integral is indeed (π/2) I_0(1).

Therefore, the original integral becomes 2^(3/2) * (π/2) I_0(1) = 2^(1/2) π I_0(1) = sqrt(2) π I_0(1).

So the exact answer is sqrt(2) π times the modified Bessel function of the first kind of order 0 evaluated at 1, which is written as √2 π I₀(1).

Now, for the numerical approximation. The modified Bessel function I₀(1) has a known value. Let me recall that I₀(1) ≈ 1.266065878. Let's compute sqrt(2) * π * 1.266065878.

First, sqrt(2) ≈ 1.41421356237, π ≈ 3.14159265359.

Multiplying these together:

1.41421356237 * 3.14159265359 ≈ 4.44288290815818

Then multiply by 1.266065878:

4.44288290815818 * 1.266065878 ≈ Let's compute this step by step.

First, 4 * 1.266065878 = 5.064263512

0.44288290815818 * 1.266065878 ≈ 0.442882908 * 1.266065878 ≈

0.4 * 1.266065878 = 0.5064263512

0.042882908 * 1.266065878 ≈ 0.042882908 * 1 = 0.042882908, 0.042882908 * 0.266065878 ≈ 0.011415, so total ≈ 0.042882908 + 0.011415 ≈ 0.054297

So total ≈ 0.5064263512 + 0.054297 ≈ 0.560723

So total approximation: 5.064263512 + 0.560723 ≈ 5.6249865

But this is a rough estimate. Let me use a calculator for more accuracy.

Alternatively, use known values. The exact value of I₀(1) is approximately 1.2660658777520084. Then sqrt(2) is approximately 1.4142135623730951. Multiply these with π:

1.4142135623730951 * 3.141592653589793 ≈ 4.442882908158084

Then multiply by 1.2660658777520084:

4.442882908158084 * 1.2660658777520084 ≈

Let's compute this:

4 * 1.2660658777520084 = 5.064263510008034

0.442882908158084 * 1.2660658777520084 ≈

0.4 * 1.2660658777520084 = 0.5064263511008034

0.042882908158084 * 1.2660658777520084 ≈

0.04 * 1.2660658777520084 = 0.05064263511008034

0.002882908158084 * 1.266065877752 ≈ 0.00365

So total ≈ 0.5064263511008034 + 0.05064263511008034 + 0.00365 ≈ 0.560719

Adding to 5.064263510008034 gives 5.6249825. But this is still approximate. Let me use a calculator for precise multiplication.

Alternatively, use a calculator: 4.442882908158084 * 1.2660658777520084

Let me compute this step by step:

First, 4 * 1.2660658777520084 = 5.064263510008034

0.4 * 1.2660658777520084 = 0.5064263511008034

0.04 * 1.2660658777520084 = 0.05064263511008034

0.002 * 1.2660658777520084 = 0.0025321317555040168

0.000882908158084 * 1.2660658777520084 ≈ 0.001117

Adding all parts:

5.064263510008034 + 0.5064263511008034 = 5.5706898611088374

+ 0.05064263511008034 = 5.621332496218918

+ 0.0025321317555040168 = 5.623864627974422

+ 0.001117 ≈ 5.624981627974422

So approximately 5.6249816. Rounded to 10 decimal places, this is approximately 5.624981627974422, which rounds to 5.6249816280.

But let me check using a calculator. Alternatively, use known value of I₀(1) and compute sqrt(2) * π * I₀(1):

I₀(1) ≈ 1.2660658777520084

sqrt(2) ≈ 1.4142135623730951

π ≈ 3.141592653589793

Multiply them:

1.4142135623730951 * 3.141592653589793 = 4.442882908158084

4.442882908158084 * 1.2660658777520084 ≈

Let me compute this multiplication precisely:

4.442882908158084 * 1.2660658777520084

Break it into 4.442882908158084 * 1 = 4.442882908158084

4.442882908158084 * 0.2 = 0.8885765816316168

4.442882908158084 * 0.06 = 0.266572974489485

4.442882908158084 * 0.006 = 0.0266572974489485

4.442882908158084 * 0.0000658777520084 ≈ 4.442882908158084 * 0.00006 = 0.000266572974489485, and 4.442882908158084 * 0.0000058777520084 ≈ ~0.0000261. So total ≈ 0.000266572974489485 + 0.0000261 ≈ 0.00029267.

Adding all parts:

4.442882908158084 + 0.8885765816316168 = 5.3314594897897

+ 0.266572974489485 = 5.598032464279185

+ 0.0266572974489485 = 5.624689761728134

+ 0.00029267 ≈ 5.624982431728134

So approximately 5.6249824317. Rounded to 10 decimal places, this is 5.6249824317. But let me check with a calculator. Alternatively, use a calculator for exact value.

Alternatively, use the known value of the integral. Wait, perhaps this integral is known. Let me check if the original integral can be expressed in terms of known constants.

Alternatively, since the exact answer is sqrt(2) π I_0(1), and I_0(1) is a known value, we can present the exact answer as √2 π I₀(1), and the numerical value as approximately 5.6249824317.

But let me verify with a numerical integration of the original integral. Let's approximate the original integral numerically to check.

The original integral is ∫0^2 x^{-1/4} (2 - x)^{-3/4} cosh( (x(2 - x))^{1/4} ) dx.

Let me approximate this numerically. Let's use substitution x = 2 sin²θ, which we did earlier. Then the integral becomes 2 ∫0^{π/2} sin^{1/2}θ cos^{-1/2}θ cosh( sqrt(sin(2θ)) ) dθ.

But integrating this might be time-consuming manually. Alternatively, use numerical approximation.

Alternatively, since we have the analytical expression as sqrt(2) π I_0(1), and I_0(1) ≈ 1.2660658777520084, then sqrt(2) * π * 1.2660658777520084 ≈ 1.4142135623730951 * 3.141592653589793 * 1.2660658777520084.

Compute 1.4142135623730951 * 3.141592653589793 ≈ 4.442882908158084.

Then 4.442882908158084 * 1.2660658777520084 ≈ 5.6249824317557175.

Rounded to 10 decimal places, this is 5.6249824318. So the numerical approximation is approximately 5.6249824318.

Therefore, the exact answer is sqrt(2) π I_0(1), and the numerical approximation is approximately 5.6249824318.
</think>

{"answer": "\\sqrt{2} \\pi I_{0}(1)", "numerical_answer": 5.6249824318}