To solve the definite integral \(\int_0^1 \lfloor \log_{2023} x \rfloor \, dx\), we follow these steps:

### Step 1: Understand the Floor Function in the Integral
The floor function \(\lfloor \log_{2023} x \rfloor\) gives the greatest integer less than or equal to \(\log_{2023} x\). 

For \(x \in (0, 1)\), \(\log_{2023} x\) is negative because \(2023 > 1\) and \(x < 1\). Let \(k = \lfloor \log_{2023} x \rfloor\), where \(k\) is a negative integer.

### Step 2: Determine the Intervals Where \(\lfloor \log_{2023} x \rfloor\) is Constant
The floor function changes its value when \(\log_{2023} x\) crosses an integer. For each integer \(k \leq -1\), we have:
\[
k \leq \log_{2023} x < k + 1
\]
This translates to:
\[
2023^k \geq x > 2023^{k+1}
\]
However, since \(k\) is negative, \(2023^{k+1} < 2023^k\).

Thus, the interval where \(\lfloor \log_{2023} x \rfloor = k\) is:
\[
x \in (2023^{k+1}, 2023^k]
\]

### Step 3: Express the Integral as a Sum
The integral can be written as a sum over all negative integers \(k\):
\[
\int_0^1 \lfloor \log_{2023} x \rfloor \, dx = \sum_{k=-\infty}^{-1} k \cdot \left(2023^k - 2023^{k+1}\right)
\]
Simplify the term inside the sum:
\[
2023^k - 2023^{k+1} = 2023^k (1 - 2023) = -2022 \cdot 2023^k
\]
Thus, the integral becomes:
\[
\sum_{k=-\infty}^{-1} k \cdot (-2022 \cdot 2023^k) = -2022 \sum_{k=-\infty}^{-1} k \cdot 2023^k
\]

### Step 4: Evaluate the Sum
Let \(S = \sum_{k=-\infty}^{-1} k \cdot 2023^k\). Substitute \(n = -k\) (so \(n \geq 1\)):
\[
S = \sum_{n=1}^{\infty} (-n) \cdot 2023^{-n} = -\sum_{n=1}^{\infty} n \cdot \left(\frac{1}{2023}\right)^n
\]
The sum \(\sum_{n=1}^{\infty} n r^n\) for \(|r| < 1\) is \(\frac{r}{(1 - r)^2}\). Here, \(r = \frac{1}{2023}\):
\[
\sum_{n=1}^{\infty} n \cdot \left(\frac{1}{2023}\right)^n = \frac{\frac{1}{2023}}{\left(1 - \frac{1}{2023}\right)^2} = \frac{2023}{(2022)^2}
\]
Thus:
\[
S = -\frac{2023}{2022^2}
\]

### Step 5: Compute the Integral
Substitute \(S\) back into the integral expression:
\[
\int_0^1 \lfloor \log_{2023} x \rfloor \, dx = -2022 \cdot S = -2022 \cdot \left(-\frac{2023}{2022^2}\right) = \frac{2023}{2022}
\]

### Step 6: Numerical Approximation
The exact answer is \(\frac{2023}{2022}\). Numerically:
\[
\frac{2023}{2022} \approx 1.0004945598
\]

### Final Answer
```json
{"answer": "\\frac{2023}{2022}", "numerical_answer": "1.0004945598"}
```