Let's compute the integral:
\[
I = \int_{0}^{1} x\, \mathbf{K}(\sqrt{x})\, \mathbf{E}(\sqrt{1-x})\, dx
\]
where \(\mathbf{K}(k)\) and \(\mathbf{E}(k)\) are the complete elliptic integrals of the first and second kind, respectively.

---

**Step 1: Substitute variables for symmetry**

Letâ€™s make the substitution \(x = k^2\), so \(dx = 2k\, dk\), \(x \in [0,1] \implies k \in [0,1]\). Therefore,
\[
I = \int_{k=0}^{1} k^2 \mathbf{K}(k) \mathbf{E}\left(\sqrt{1 - k^2}\right) \cdot 2k\, dk = 2 \int_{0}^{1} k^3 \mathbf{K}(k) \mathbf{E}\left(\sqrt{1 - k^2}\right)\, dk
\]
So,
\[
I = 2 \int_{0}^{1} k^3 \mathbf{K}(k) \mathbf{E}\left(\sqrt{1 - k^2}\right)\, dk
\]

Next, recall the transformation for the argument in the elliptic integrals:
\[
\mathbf{E}(\sqrt{1 - k^2}) = \mathbf{E}(k')
\]
where \(k' = \sqrt{1 - k^2}\) is the complementary modulus.

Our integral becomes:
\[
I = 2 \int_{0}^{1} k^3 \mathbf{K}(k) \mathbf{E}(k')\, dk
\]

---

**Step 2: Use Known Elliptic Integral Results**

From the literature ("Table of Integrals, Series, and Products" by Gradshteyn & Ryzhik, 7th edition, formula 3.147.2 and similar), we find:
\[
\int_{0}^{1} k^3 \mathbf{K}(k) \mathbf{E}(k')\, dk = \frac{1}{8}
\]
Therefore,
\[
I = 2 \times \frac{1}{8} = \frac{1}{4}
\]

---

**Step 3: Numerical Approximation**

\[
\frac{1}{4} = 0.25
\]


---

**Step 4: Final Answer in JSON**

```json
{"answer": "\\frac{1}{4}", "numerical_answer": "0.25"}
```