

To calculate the definite integral \(\int_1^2 \left(2^{x-1} + \log_2(2x)\right) \, dx\), we proceed as follows:

### Step 1: Split the integral into two parts
The integral is linear, so we split it into two separate integrals:
\[
\int_1^2 2^{x-1} \, dx + \int_1^2 \log_2(2x) \, dx
\]

### Step 2: Evaluate the first integral \(\int_1^2 2^{x-1} \, dx\)
The integral of \(2^{x-1}\) with respect to \(x\) is found using the formula for integrating exponential functions. Recall that \(\int a^u \, du = \frac{a^u}{\ln a} + C\) for \(a > 0\), \(a \neq 1\). Here, \(u = x - 1\), so \(du = dx\). Thus:
\[
\int 2^{x-1} \, dx = \frac{2^{x-1}}{\ln 2} + C
\]
Evaluating from \(1\) to \(2\):
\[
\left. \frac{2^{x-1}}{\ln 2} \right|_1^2 = \frac{2^{2-1}}{\ln 2} - \frac{2^{1-1}}{\ln 2} = \frac{2}{\ln 2} - \frac{1}{\ln 2} = \frac{1}{\ln 2}
\]

### Step 3: Evaluate the second integral \(\int_1^2 \log_2(2x) \, dx\)
First, simplify \(\log_2(2x)\) using logarithm properties: \(\log_2(2x) = \log_2(2) + \log_2(x) = 1 + \log_2(x)\). Thus, the integral becomes:
\[
\int_1^2 \left(1 + \log_2(x)\right) \, dx = \int_1^2 1 \, dx + \int_1^2 \log_2(x) \, dx
\]

#### Substep 3.1: Evaluate \(\int_1^2 1 \, dx\)
This is straightforward:
\[
\int_1^2 1 \, dx = \left. x \right|_1^2 = 2 - 1 = 1
\]

#### Substep 3.2: Evaluate \(\int_1^2 \log_2(x) \, dx\)
Convert \(\log_2(x)\) to natural logarithms: \(\log_2(x) = \frac{\ln x}{\ln 2}\). Thus:
\[
\int \log_2(x) \, dx = \frac{1}{\ln 2} \int \ln x \, dx
\]
The integral of \(\ln x\) is \(x \ln x - x + C\), so:
\[
\int \log_2(x) \, dx = \frac{1}{\ln 2} \left( x \ln x - x \right) + C
\]
Evaluating from \(1\) to \(2\):
\[
\left. \frac{1}{\ln 2} \left( x \ln x - x \right) \right|_1^2 = \frac{1}{\ln 2} \left[ (2 \ln 2 - 2) - (1 \ln 1 - 1) \right]
\]
Since \(\ln 1 = 0\), this simplifies to:
\[
\frac{1}{\ln 2} \left[ (2 \ln 2 - 2) - (-1) \right] = \frac{1}{\ln 2} \left( 2 \ln 2 - 1 \right)
\]

#### Substep 3.3: Combine results for the second integral
Adding the two parts of the second integral:
\[
1 + \frac{1}{\ln 2} \left( 2 \ln 2 - 1 \right) = 1 + 2 - \frac{1}{\ln 2} = 3 - \frac{1}{\ln 2}
\]

### Step 4: Combine both integrals
Adding the results of the first and second integrals:
\[
\frac{1}{\ln 2} + \left( 3 - \frac{1}{\ln 2} \right) = 3
\]

### Numerical Approximation
The exact result is \(3\), so the numerical approximation is \(3.0000000000\).

{"answer": "3", "numerical_answer": "3.0000000000"}