Let's begin by carefully analyzing the integral:

\[
I = \int_0^{2} x^{-3/4} (2-x)^{-1/4} I_1\left( 1 \cdot \sqrt[4]{x(2-x)} \right) dx
\]

where \( I_1 \) is the modified Bessel function of the first kind.

---

## Step 1: Substitution

Let us substitute \( x = 2 t \), so when \( x = 0 \), \( t = 0 \) and when \( x = 2 \), \( t = 1 \).
Then \( dx = 2 dt \).

Now,
\[
x^{-3/4} = (2 t)^{-3/4} = 2^{-3/4} t^{-3/4}
\]
\[
2-x = 2 - 2t = 2(1-t)
\implies (2-x)^{-1/4} = [2(1-t)]^{-1/4} = 2^{-1/4} (1-t)^{-1/4}
\]

Also,
\[
x(2-x) = 2t \cdot 2(1-t) = 4t(1-t)
\implies \sqrt[4]{x(2-x)} = \sqrt[4]{4 t (1-t)} = 4^{1/4} (t(1-t))^{1/4} = 2^{1/2} (t(1-t))^{1/4}
\]

So the argument of the Bessel function is \( 1 \cdot 2^{1/2} (t(1-t))^{1/4} = \sqrt{2} (t(1-t))^{1/4} \).

Now, combining all:

\[
I = \int_{t=0}^{t=1} \left[2^{-3/4} t^{-3/4}\right] \left[2^{-1/4} (1-t)^{-1/4}\right] I_1\left(\sqrt{2}(t(1-t))^{1/4}\right) \cdot 2 dt
\]

Multiply constants:
\[
2^{-3/4} \cdot 2^{-1/4} \cdot 2 = 2^{-1} \cdot 2 = 1
\]

So the integral reduces to:
\[
I = \int_0^1 t^{-3/4} (1-t)^{-1/4} I_1\left(\sqrt{2}(t(1-t))^{1/4}\right) dt
\]

---

## Step 2: Series Expansion for \( I_1 \)

Recall:
\[
I_1(z) = \sum_{k=0}^\infty \frac{1}{k! \Gamma(k+2)} \left( \frac{z}{2} \right)^{2k+1}
\]

Set \( z = \sqrt{2} (t(1-t))^{1/4} \):

So,
\[
I_1\left(\sqrt{2} (t(1-t))^{1/4}\right) = \sum_{k=0}^{\infty} \frac{1}{k! \Gamma(k+2)} \left( \frac{\sqrt{2}}{2} (t(1-t))^{1/4} \right)^{2k+1}
\]
But \( \frac{\sqrt{2}}{2} = 2^{-1/2} \), so

\[
\left[ 2^{-1/2} (t(1-t))^{1/4} \right]^{2k+1} 
= 2^{-(2k+1)/2} (t(1-t))^{(2k+1)/4}
\]

So,

\[
I_1\left(\sqrt{2} (t(1-t))^{1/4}\right) = \sum_{k=0}^{\infty} \frac{2^{-(2k+1)/2}}{k! \Gamma(k+2)} (t(1-t))^{(2k+1)/4}
\]

---

Now, plug back into the integral:

\[
I = \int_0^1 t^{-3/4} (1-t)^{-1/4} \sum_{k=0}^{\infty} \frac{2^{-(2k+1)/2}} {k! \Gamma(k+2)} (t(1-t))^{(2k+1)/4} dt
\]

Switch sum and integral (since all terms are positive in [0,1]),

\[
I = \sum_{k=0}^{\infty} \frac{2^{-(2k+1)/2}} {k! \Gamma(k+2)} \int_0^1 t^{-3/4 + (2k+1)/4}(1-t)^{-1/4 + (2k+1)/4} dt
\]

\[
-3/4 + (2k+1)/4 = \frac{-3 + 2k + 1}{4} = \frac{2k - 2}{4} = \frac{k-1}{2}
\]
\[
-1/4 + (2k+1)/4 = \frac{-1 + 2k + 1}{4} = \frac{2k}{4} = \frac{k}{2}
\]

So,

\[
I = \sum_{k=0}^{\infty} \frac{2^{-(2k+1)/2}} {k! \Gamma(k+2)} \int_0^1 t^{(k-1)/2} (1-t)^{k/2} dt
\]

But

\[
\int_0^1 t^{a-1} (1-t)^{b-1} dt = \mathrm{B}(a, b) = \frac{\Gamma(a)\Gamma(b)} {\Gamma(a+b)}
\]

Set
\[
a = \frac{k+1}{2},\qquad b = \frac{k+2}{2}
\]

So,

\[
I = \sum_{k=0}^{\infty} \frac{2^{-(2k+1)/2}}{k! \Gamma(k+2)} \cdot \frac{\Gamma\left(\frac{k+1}{2}\right) \Gamma\left(\frac{k+2}{2}\right)}{\Gamma(k+1.5)}
\]

---

### Step 3: Closed-form Expression

So, the integral evaluates exactly to

\[
I = \sum_{k=0}^{\infty} \frac{2^{-(2k+1)/2}\; \Gamma\left(\frac{k+1}{2}\right) \Gamma\left(\frac{k+2}{2}\right)}{k! \, \Gamma(k+2)\, \Gamma(k+1.5)}
\]
or, more simply,

\[
I = \sum_{k=0}^{\infty} \frac{2^{-(2k+1)/2}\; \Gamma\left(\frac{k+1}{2}\right) \Gamma\left(\frac{k+2}{2}\right)}{k! \, \Gamma(k+2)\, \Gamma(k+\frac{3}{2})}
\]

---

## Step 4: Numerical evaluation

Let's numerically evaluate the sum for several terms.

We will calculate the first few terms:

Letâ€™s compute for \( k = 0, 1, 2, 3, 4, 5 \):

- For \( k = 0 \):

  - \( 2^{-(1)/2} = 2^{-0.5} = 1/\sqrt{2} \)
  - \( \Gamma(0+1)/2 = \Gamma(0.5) = \sqrt{\pi} \)
  - \( \Gamma(0+2)/2 = \Gamma(1) = 1 \)
  - \( k! = 1 \)
  - \( \Gamma(2) = 1! = 1 \)
  - \( \Gamma(1.5) = \frac{\sqrt{\pi}}{2} \)
  
  So,
  \[
  T_0 = \frac{1/\sqrt{2} \cdot \sqrt{\pi}\cdot 1}{1 \cdot 1 \cdot (\sqrt{\pi}/2)} = \frac{1}{\sqrt{2}} \cdot \frac{\sqrt{\pi}}{\sqrt{\pi}/2} = \frac{1}{\sqrt{2}} \cdot 2 = \frac{2}{\sqrt{2}} = \sqrt{2} \approx 1.4142135624
  \]

- For \( k = 1 \):

  - \( 2^{-(3)/2} = 2^{-1.5} = 1/ (2 \sqrt{2}) \)
  - \( \Gamma(1) = 1 \)
  - \( \Gamma(1.5) = \sqrt{\pi}/2 \)
  - \( k! = 1 \)
  - \( \Gamma(3) = 2 \)
  - \( \Gamma(2.5) = \frac{3 \sqrt{\pi}}{4} \)
  
  So,
  \[
  T_1 = \frac{1/(2 \sqrt{2}) \cdot 1 \cdot (\sqrt{\pi}/2)}{1 \cdot 2 \cdot (3 \sqrt{\pi}/4)}
  \]
  Numerators: \( 1 \cdot 1 \cdot (\sqrt{\pi}/2) = \sqrt{\pi}/2 \)
  
  Denominator: \( 1 \cdot 2 \cdot (3 \sqrt{\pi} / 4) = 2 \cdot (3/4) \cdot \sqrt{\pi} = (3/2) \sqrt{\pi}  \)

So overall,

\[
T_1 = \frac{1}{2 \sqrt{2}} \cdot \frac{1}{2} \cdot \frac{\sqrt{\pi}}{(3/2) \sqrt{\pi}} = \frac{1}{2 \sqrt{2}} \cdot \frac{1}{2} \cdot \frac{1}{3/2}
\]
First, \( \sqrt{\pi}/\sqrt{\pi} = 1 \).
So,

\[
T_1 = \frac{1}{2\sqrt{2}} \cdot \frac{1}{2} \cdot \frac{2}{3}
= \frac{1}{2\sqrt{2}} \cdot \frac{1}{3}
= \frac{1}{6\sqrt{2}} \approx \frac{1}{6 \times 1.41421356} \approx \frac{1}{8.4852814} \approx 0.1178511302
\]

- For \( k = 2 \):

  - \( 2^{-(5)/2} = 2^{-2.5} = 1/(4\sqrt{2}) \)
  - \( \Gamma(1.5) = \sqrt{\pi}/2 \)
  - \( \Gamma(2) = 1 \)
  - \( (2)! = 2 \)
  - \( \Gamma(4) = 6 \)
  - \( \Gamma(3.5) = \frac{3 \cdot 5 \sqrt{\pi}}{4 \cdot 8} = \frac{15 \sqrt{\pi}}{32} \)
  
  Focusing on the main calculation:

Numerator: \( 1/(4\sqrt{2}) \cdot (\sqrt{\pi}/2) \cdot 1 = (\sqrt{\pi})/(8\sqrt{2}) \)
  
Denominator: \( 2 \cdot 6 \cdot (15 \sqrt{\pi}/32) = 12 \cdot (15/32) \sqrt{\pi} = (180/32) \sqrt{\pi} = (45/8) \sqrt{\pi} \)

So,

\[
T_2 = \frac{(\sqrt{\pi})/(8\sqrt{2})}{(45/8)\sqrt{\pi}}
= \frac{1}{8\sqrt{2}} \cdot \frac{8}{45}
= \frac{1}{\sqrt{2}} \cdot \frac{1}{45}
= \frac{1}{45 \cdot 1.41421356} \approx \frac{1}{63.6396102} \approx 0.0157152760
\]

- For \(k=3\):

  - \(2^{-(7)/2} = 2^{-3.5} = 1/(8\sqrt{2})\)
  - \(\Gamma(2) = 1\)
  - \(\Gamma(2.5) = 1.329340388\)
  - \(3! = 6\)
  - \(\Gamma(5) = 24\)
  - \(\Gamma(4.5) = 11.63172840\)
  
Numerator: \(1/(8\sqrt{2}) \cdot 1 \cdot 1.329340388 = 1.329340388/(8\sqrt{2})\)

Denominator: \(6 \cdot 24 \cdot 11.63172840 = 144 \cdot 11.63172840 = 1676.967\)

So

\[
T_3 = \frac{1.329340388}{8\sqrt{2}\cdot 1676.967}
= \frac{1.329340388}{8 \cdot 1.41421356 \cdot 1676.967}
= \frac{1.329340388}{13,570.20}
\approx 0.0000979581
\]

- For \(k=4\):

  - \(2^{-(9)/2} = 2^{-4.5} = 1/(16\sqrt{2})\)
  - \(\Gamma(2.5) = 1.329340388\)
  - \(\Gamma(3) = 2\)
  - \(4! = 24\)
  - \(\Gamma(6) = 120\)
  - \(\Gamma(5.5) = 52.34277778\)

Numerator: \(1.329340388 \cdot 2 / (16\sqrt{2}) = 2.658680776/(16\sqrt{2})\)
Denominator: \(24 \cdot 120 \cdot 52.34277778 = 2880 \cdot 52.34277778 = 150,549.634\)

So,

\[
T_4 = \frac{2.658680776}{16 \cdot 1.41421356 \cdot 150,549.634}
= \frac{2.658680776}{3,395,570.25}
\approx 0.0000007833
\]

The terms become exceedingly small.

Summing up:

\[
I \approx T_0 + T_1 + T_2 + T_3 + T_4
\]
\[
I \approx 1.4142135624 + 0.1178511302 + 0.0157152760 + 0.0000979581 + 0.0000007833
\approx 1.547878710
\]

To get 10 digits, let's add the next term (\(k=5\)):

- \(2^{-(11)/2} = 2^{-5.5} = 1/(32\sqrt{2}) = 0.0220970869\)
- \(\Gamma(3) = 2\)
- \(\Gamma(3.5) = 3.323350970\)
- \(5! = 120\)
- \(\Gamma(7) = 720\)
- \(\Gamma(6.5) = 287.8852778\)

Numerator: \(2 \cdot 3.323350970 / (32\sqrt{2}) = 6.64670194/(32 \cdot 1.41421356) = 6.64670194/45.2542377 = 0.146887928\)

Denominator: \(120 \cdot 720 \cdot 287.8852778 = 86,400 \cdot 287.8852778 = 24,880,114.2\)

\(T_5 = 0.146887928 / 24,880,114.2 = 5.904 \times 10^{-9}\)

Adding, has almost no effect.

So

\[
I \approx 1.547878710
\]

---

### Step 5: Final Exact and Numerical Answers

**Exact expression in LaTeX:**

\[
I = \sum_{k=0}^{\infty} \frac{2^{-(2k+1)/2}\; \Gamma\left(\frac{k+1}{2}\right) \Gamma\left(\frac{k+2}{2}\right)}{k! \, \Gamma(k+2)\, \Gamma(k+\frac{3}{2})}
\]

**Numerical approximation (rounded to 10 decimal places):**

\[
I \approx 1.5478787100
\]

---

## JSON Answer

```json
{"answer": "\\sum_{k=0}^{\\infty} \\frac{2^{-(2k+1)/2}\\; \\Gamma\\left(\\frac{k+1}{2}\\right) \\Gamma\\left(\\frac{k+2}{2}\\right)}{k! \\, \\Gamma(k+2)\\, \\Gamma(k+\\frac{3}{2})}", "numerical_answer": "1.5478787100"}
```