<think>
Okay, so I need to compute the definite integral from 1 to 2011 of sqrt(x) divided by (sqrt(2012 - x) + sqrt(x)) dx. Hmm, let's see. I remember that sometimes when you have integrals with symmetric terms in the denominator, a substitution might help simplify things. Let me think about possible substitutions here.

The denominator has sqrt(2012 - x) and sqrt(x). Maybe if I let t = 2012 - x, that could swap the terms. Let's try that substitution. If t = 2012 - x, then when x = 1, t = 2011, and when x = 2011, t = 1. Also, dx = -dt. So the integral becomes:

Integral from t=2011 to t=1 of sqrt(2012 - t) / (sqrt(t) + sqrt(2012 - t)) * (-dt). Flipping the limits to remove the negative sign, it becomes the integral from 1 to 2011 of sqrt(2012 - t) / (sqrt(t) + sqrt(2012 - t)) dt.

But the original integral is of sqrt(x)/(sqrt(2012 - x) + sqrt(x)) dx. If I denote the original integral as I, then after substitution, the new integral is the same as I but with sqrt(2012 - t) in the numerator. So if I add the original integral I and the substituted integral, I get:

I + I = integral from 1 to 2011 of [sqrt(x) + sqrt(2012 - x)] / [sqrt(2012 - x) + sqrt(x)] dx.

The numerator and denominator are the same, so this simplifies to the integral of 1 dx from 1 to 2011. That integral is just (2011 - 1) = 2010. Therefore, 2I = 2010, so I = 2010 / 2 = 1005. Wait, that seems too straightforward. Let me check again.

Original integral: I = ∫₁²⁰¹¹ [sqrt(x)/(sqrt(2012 - x) + sqrt(x))] dx.

After substitution t = 2012 - x, the integral becomes ∫₁²⁰¹¹ [sqrt(2012 - t)/(sqrt(t) + sqrt(2012 - t))] dt. Let's call this integral J. Then I + J = ∫₁²⁰¹¹ [sqrt(x) + sqrt(2012 - x)] / [sqrt(x) + sqrt(2012 - x)] dx = ∫₁²⁰¹¹ 1 dx = 2010. Since I and J are the same integral (because substitution just renames the variable), then I = J. Therefore, 2I = 2010, so I = 1005. That makes sense. So the exact answer is 1005. Then the numerical approximation is just 1005.0000000000. Let me confirm with a simple case. Suppose the integral from a to b of sqrt(x)/(sqrt(c - x) + sqrt(x)) dx, where c = a + b. Then using the same substitution, t = c - x, the same steps would apply, leading to (b - a)/2. In this case, a=1, b=2011, c=2012. So (2011 -1)/2 = 2010/2 = 1005. Yep, that checks out. So the answer is 1005 exactly. The numerical approximation is 1005.0000000000.
</think>

{"answer": "1005", "numerical_answer": "1005.0000000000"}