Let's compute the integral:
\[
I = \int_{0}^{1/2} \ln\left(\sqrt{1-x} - \sqrt{x}\right) \, dx
\]

---

**Step 1: Simplify the Integrand**

First, notice that \(\sqrt{1-x} - \sqrt{x}\) is positive for \(0 \leq x < \frac{1}{2}\), so the logarithm is defined on this interval.

Let us try the substitution:
\[
x = \sin^2 \theta,\quad dx = 2\sin\theta \cos\theta \, d\theta = \sin 2\theta \, d\theta,\quad x \in [0, 1/2] \implies \theta \in [0, \arcsin(1/\sqrt{2})] = [0, \pi/4]
\]
Now:
\[
\sqrt{1-x} - \sqrt{x} = \sqrt{1-\sin^2 \theta} - \sin \theta = \cos \theta - \sin \theta
\]
Thus:
\[
I = \int_{x=0}^{x=1/2} \ln(\cos\theta - \sin\theta) \cdot dx
\]
Recall for bounds:

- When \(x=0\), \(\theta = 0\)
- When \(x=1/2\), \(\sin \theta = 1/\sqrt{2} \implies \theta = \pi/4\)

Remember that \(dx = \sin 2\theta d\theta\):

So:
\[
I = \int_{0}^{\pi/4} \ln(\cos\theta - \sin\theta) \cdot \sin 2\theta\, d\theta
\]
But \(\sin 2\theta = 2\sin\theta \cos\theta\), so:
\[
I = \int_{0}^{\pi/4} \ln(\cos\theta - \sin\theta) \cdot 2\sin\theta\cos\theta\, d\theta
\]

Alternatively, expressing \(\cos\theta - \sin\theta\) as a single sine function:
\[
\cos\theta - \sin\theta = \sqrt{2} \sin\left( \frac{\pi}{4} - \theta \right )
\]

Let's use this:
\[
I = \int_{0}^{\pi/4} \ln \left( \sqrt{2} \sin \left( \frac{\pi}{4} - \theta \right ) \right ) \cdot \sin 2\theta\, d\theta
\]

Recall \(\sin 2\theta = 2\sin\theta \cos\theta\), but we can also leave it as is for now.

Expand the logarithm:
\[
\ln \left( \sqrt{2} \sin \left( \frac{\pi}{4} - \theta \right ) \right ) = \frac{1}{2}\ln 2 + \ln \sin \left( \frac{\pi}{4} - \theta \right )
\]

Therefore,
\[
I = \int_{0}^{\pi/4} \left( \frac{1}{2}\ln 2 + \ln \sin \left( \frac{\pi}{4} - \theta \right ) \right ) \sin 2\theta\, d\theta
\]
\[
= \frac{1}{2}\ln 2 \int_{0}^{\pi/4} \sin 2\theta \, d\theta + \int_{0}^{\pi/4} \ln \sin \left( \frac{\pi}{4} - \theta \right ) \sin 2\theta \, d\theta
\]

Let's compute both terms.

---

**Step 2: Evaluate Each Integral**

**First integral:**
\[
I_1 = \int_{0}^{\pi/4} \sin 2\theta \, d\theta
\]
Let \(u = 2\theta\), so \(du = 2 d\theta\) or \(d\theta = du/2\):

- When \(\theta = 0\), \(u = 0\)
- When \(\theta = \pi/4\), \(u = \pi/2\)

Thus:
\[
I_1 = \int_{u=0}^{u=\pi/2} \sin u \cdot \frac{du}{2} = \frac{1}{2} \int_{0}^{\pi/2} \sin u\, du = \frac{1}{2} [ -\cos u ]_{0}^{\pi/2} = \frac{1}{2} ( -\cos(\pi/2) + \cos(0) ) = \frac{1}{2} (0 + 1) = \frac{1}{2}
\]

So the first term is:
\[
\frac{1}{2}\ln 2 \cdot \frac{1}{2} = \frac{1}{4} \ln 2
\]

---

**Second integral:**
\[
I_2 = \int_{0}^{\pi/4} \ln \sin \left( \frac{\pi}{4} - \theta \right ) \sin 2\theta \, d\theta
\]

Let \(u = \frac{\pi}{4} - \theta\), then \(\theta = \frac{\pi}{4} - u\), as \(\theta\) increases from \(0\) to \(\pi/4\), \(u\) decreases from \(\frac{\pi}{4}\) to \(0\):

But let's change the direction so that the limits go from 0 to \(\pi/4\):

If \(u\) goes \( \frac{\pi}{4} \to 0\), then \(du = -d\theta\).

So,
\[
I_2 = \int_{\theta=0}^{\theta=\pi/4} \ln \sin \left( \frac{\pi}{4} - \theta \right ) \sin 2\theta\, d\theta = \int_{u=\pi/4}^{u=0} \ln \sin u \cdot \sin 2(\pi/4 - u) \cdot ( - du )
\]
\[
= \int_{u=0}^{u=\pi/4} \ln \sin u \cdot \sin 2(\pi/4 - u)\, du
\]

Now, expand \(\sin(2(\pi/4-u))\):

\[
2(\pi/4 - u) = \frac{\pi}{2} - 2u
\]
so
\[
\sin(2(\pi/4 - u)) = \sin\left(\frac{\pi}{2} - 2u\right) = \cos(2u)
\]

Therefore,
\[
I_2 = \int_0^{\pi/4} \ln\sin u \cdot \cos(2u) \, du
\]

---

**Step 3: Put It All Together**

Thus, the original integral simplifies to:

\[
I = \frac{1}{4}\ln 2 + \int_0^{\pi/4} \ln\sin u \cdot \cos (2u) du
\]

---

**Step 4: Compute the Integral \(\displaystyle \int_0^{\pi/4} \ln\sin u \cdot \cos 2u \, du\)**

We can write:
\[
\int_{0}^{\pi/4} \ln \sin u \cos 2u\, du
\]
Let us express \(\cos 2u\) as \(2\cos^2 u - 1\). But more directly, let's try integrating by parts.

Letâ€™s use integration by parts:

Let \(f(u) = \ln \sin u\), \(dg = \cos 2u \, du\), then \(df = \cot u \, du\), \(g(u) = \frac{1}{2} \sin 2u\).

Then,

\[
\int \ln \sin u \cdot \cos 2u \, du = \ln \sin u \cdot \frac{1}{2} \sin 2u - \int \frac{1}{2} \sin 2u \cdot \cot u\, du
\]

Now,
\[
\sin 2u = 2\sin u \cos u
\]
and
\[
\cot u = \frac{\cos u}{\sin u}
\]
So,
\[
\sin 2u \cdot \cot u = 2\sin u \cos u \cdot \frac{\cos u}{\sin u} = 2\cos^2 u
\]
Therefore,
\[
\int \ln \sin u \cdot \cos 2u \, du = \frac{1}{2} \ln \sin u \cdot \sin 2u - \int \cos^2 u\, du
\]

Recall,
\[
\cos^2 u = \frac{1 + \cos 2u}{2}
\]
Thus,
\[
\int \cos^2 u \, du = \int \frac{1 + \cos 2u}{2} du = \frac{1}{2} \int du + \frac{1}{2} \int \cos 2u du = \frac{u}{2} + \frac{1}{4}\sin 2u
\]

Therefore,
\[
\int \ln \sin u \cdot \cos 2u du = \frac{1}{2} \ln \sin u \cdot \sin 2u - \frac{u}{2} - \frac{1}{4} \sin 2u + C
\]

Now, evaluate from \(u = 0\) to \(u = \pi/4\):

When \(u = \pi/4\):

- \(\sin u = \sin (\pi/4) = 1/\sqrt{2}\)
- \(\ln \sin u = -\frac{1}{2}\ln 2\)
- \(\sin 2u = \sin (\pi/2) = 1\)

So,
- \( \frac{1}{2} \ln \sin (\pi/4) \cdot \sin 2(\pi/4) = \frac{1}{2} \left ( -\frac{1}{2} \ln 2 \right ) \cdot 1 = -\frac{1}{4} \ln 2 \)
- \(- \frac{ u }{2 } = - \frac{ \pi }{8 } \)
- \(-\frac{1}{4} \sin 2u = -\frac{1}{4} \cdot 1 = -\frac{1}{4}\)

When \(u=0\):

- \(\sin(0) = 0 \implies \ln 0 \to -\infty \), but it's multiplied by \(\sin 0 = 0\), so indeterminate, take the limit:

\[
\lim_{u \to 0^+} \frac{1}{2} \ln \sin u \cdot \sin 2u = \lim_{u \to 0} \frac{1}{2} \ln \sin u \cdot 2u 
\]
Expand \(\sin u \sim u\) as \(u \to 0\):

\[
\ln \sin u \sim \ln u
\]
Thus,

\[
\lim_{u\to 0} \ln u \cdot 2u = 0
\]
Therefore, the first term at \(u=0\) is 0.

- \(-\frac{u}{2} = 0\)
- \(-\frac{1}{4} \sin 2u = 0\)

Therefore, at \(u=0\), the sum is 0.

So the definite value is just the upper limit:

\[
I_2 = -\frac{1}{4}\ln 2 - \frac{\pi}{8} - \frac{1}{4}
\]

---

**Step 5: Sum Both Parts for the Final Answer**

Recall:
\[
I = \frac{1}{4} \ln 2 + I_2 = \frac{1}{4} \ln 2 - \frac{1}{4}\ln 2 - \frac{\pi}{8} - \frac{1}{4} = -\frac{\pi}{8} - \frac{1}{4}
\]

Thus,
\[
\boxed{I = -\frac{1}{4} - \frac{\pi}{8}}
\]

---

**Step 6: Numerical Approximation (to 10 decimal places)**

First, compute \(\pi/8\):

\[
\pi \approx 3.141592653589793
\]
\[
\frac{\pi}{8} \approx \frac{3.141592653589793}{8} \approx 0.3926990817
\]
Therefore,
\[
I \approx -\frac{1}{4} - 0.3926990817 = -0.25 - 0.3926990817 = -0.6426990817
\]

---

**Step 7: Format the Answer as Requested**

```json
{"answer": "-\\frac{1}{4} - \\frac{\\pi}{8}", "numerical_answer": "-0.6426990817"}
```