To evaluate the definite integral

$$
\int_0^{2} x^{-3/4} (2 - x)^{-1/4} I_1\left(\sqrt[4]{x(2 - x)}\right) \, dx,
$$

we begin by analyzing the structure of the integrand. It involves powers of $ x $ and $ 2 - x $, and a modified Bessel function $ I_1 $ of the fourth root of the product $ x(2 - x) $. This suggests that the integral might be expressible in terms of special functions or known identities involving Bessel functions.

---

### Step 1: Substitution and Series Expansion

We start by using the substitution $ x = 2t $, which transforms the integral into:

$$
\int_0^1 t^{-3/4} (1 - t)^{-1/4} I_1\left(\sqrt{2} \cdot \sqrt[4]{t(1 - t)}\right) dt.
$$

We then expand the modified Bessel function $ I_1(z) $ using its series representation:

$$
I_1(z) = \sum_{k=0}^\infty \frac{(z/2)^{2k+1}}{k! (k+1)!}.
$$

Substituting $ z = \sqrt{2} \cdot \sqrt[4]{t(1 - t)} $, we obtain:

$$
I_1\left(\sqrt{2} \cdot \sqrt[4]{t(1 - t)}\right) = \sum_{k=0}^\infty \frac{(1)^{2k+1}}{k! (k+1)!} \cdot \left(\sqrt{t(1 - t)}\right)^{2k+1}.
$$

Substituting this into the integral and interchanging the sum and integral (justified by uniform convergence), we get:

$$
\int_0^1 t^{-3/4} (1 - t)^{-1/4} \sum_{k=0}^\infty \frac{\left(\sqrt{t(1 - t)}\right)^{2k+1}}{k! (k+1)!} dt
= \sum_{k=0}^\infty \frac{1}{k! (k+1)!} \int_0^1 t^{-3/4 + k + 1/2} (1 - t)^{-1/4 + k + 1/2} dt.
$$

Simplifying the exponents:

$$
t^{-3/4 + k + 1/2} = t^{k - 1/4}, \quad (1 - t)^{-1/4 + k + 1/2} = (1 - t)^{k + 1/4}.
$$

Thus, the integral becomes:

$$
\sum_{k=0}^\infty \frac{1}{k! (k+1)!} \int_0^1 t^{k - 1/4} (1 - t)^{k + 1/4} dt.
$$

This is a standard Beta function integral:

$$
\int_0^1 t^{a-1} (1 - t)^{b-1} dt = B(a, b) = \frac{\Gamma(a)\Gamma(b)}{\Gamma(a + b)}.
$$

So the integral becomes:

$$
\sum_{k=0}^\infty \frac{\Gamma(k + 3/4)\Gamma(k + 5/4)}{k! (k+1)! \Gamma(2k + 2)}.
$$

This series converges rapidly and can be evaluated numerically to high precision.

---

### Step 2: Numerical Approximation

Computing the first few terms of the series gives:

- $ k = 0 $: $ \frac{\Gamma(3/4)\Gamma(5/4)}{0! \cdot 1! \cdot \Gamma(2)} = \frac{\Gamma(3/4)\Gamma(5/4)}{1} \approx 2 $
- $ k = 1 $: $ \frac{\Gamma(7/4)\Gamma(9/4)}{1! \cdot 2! \cdot \Gamma(4)} \approx 1/6 $
- $ k = 2 $: $ \frac{\Gamma(11/4)\Gamma(13/4)}{2! \cdot 3! \cdot \Gamma(6)} \approx 1/180 $

Higher terms decay rapidly. Summing the first few terms and multiplying by