


To solve the definite integral \(\int_{0}^{2} x^{-1/2}(2-x)^{-1/2} \cosh\left(\sqrt{x(2-x)}\right) \, dx\), we proceed as follows:

### Step 1: Substitution
Let \( x = 1 + \sin\theta \). Then:
- \( 2 - x = 1 - \sin\theta \), so \( x(2-x) = (1+\sin\theta)(1-\sin\theta) = 1 - \sin^2\theta = \cos^2\theta \).
- \( \sqrt{x(2-x)} = \cos\theta \).
- \( dx = \cos\theta \, d\theta \).

The limits of integration change:
- When \( x = 0 \), \( \sin\theta = -1 \) (so \( \theta = -\pi/2 \)).
- When \( x = 2 \), \( \sin\theta = 1 \) (so \( \theta = \pi/2 \)).

### Step 2: Simplify the Integrand
Substituting into the integral:
\[
\int_{0}^{2} \frac{\cosh\left(\sqrt{x(2-x)}\right)}{\sqrt{x(2-x)}} \, dx = \int_{-\pi/2}^{\pi/2} \frac{\cosh(\cos\theta)}{\cos\theta} \cdot \cos\theta \, d\theta = \int_{-\pi/2}^{\pi/2} \cosh(\cos\theta) \, d\theta.
\]

### Step 3: Exploit Symmetry
Since \( \cosh(\cos\theta) \) is even in \( \theta \), the integral over \( [-\pi/2, \pi/2] \) equals twice the integral over \( [0, \pi/2] \):
\[
\int_{-\pi/2}^{\pi/2} \cosh(\cos\theta) \, d\theta = 2 \int_{0}^{\pi/2} \cosh(\cos\theta) \, d\theta.
\]

### Step 4: Relate to Modified Bessel Function
Using the identity \( \cosh(z) = \frac{e^z + e^{-z}}{2} \), we rewrite the integral:
\[
2 \int_{0}^{\pi/2} \cosh(\cos\theta) \, d\theta = \int_{0}^{\pi/2} \left( e^{\cos\theta} + e^{-\cos\theta} \right) d\theta.
\]

The integral \( \int_{0}^{\pi} e^{z \cos\theta} d\theta = \pi I_0(z) \), where \( I_0(z) \) is the modified Bessel function of the first kind of order 0. Splitting \( \int_{0}^{\pi} e^{\cos\theta} d\theta \) into \( \int_{0}^{\pi/2} e^{\cos\theta} d\theta + \int_{\pi/2}^{\pi} e^{\cos\theta} d\theta \) and substituting \( \phi = \pi - \theta \) in the second term shows:
\[
\int_{0}^{\pi} e^{\cos\theta} d\theta = \int_{0}^{\pi/2} \left( e^{\cos\theta} + e^{-\cos\theta} \right) d\theta.
\]

Thus, the original integral simplifies to:
\[
\int_{0}^{2} x^{-1/2}(2-x)^{-1/2} \cosh\left(\sqrt{x(2-x)}\right) \, dx = \pi I_0(1).
\]

### Step 5: Numerical Approximation
The modified Bessel function \( I_0(1) \approx 1.26606587775 \). Multiplying by \( \pi \):
\[
\pi I_0(1) \approx 3.14159265359 \times 1.26606587775 \approx 3.9774630231.
\]

### Final Answer
The exact answer is \( \pi I_0(1) \), and the numerical approximation is \( 3.9774630231 \).

{"answer": "\(\pi I_0(1)\)", "numerical_answer": "3.9774630231"}