To compute the definite integral \(\int_0^1 \frac{\ln\left(x + x^{-1}\right)}{x + x^{-1}} \, dx\), we follow these steps:

1. **Simplify the Integrand**:
   Rewrite the integrand using algebraic manipulation:
   \[
   \frac{\ln\left(\frac{x^2 + 1}{x}\right)}{\frac{x^2 + 1}{x}} \cdot \frac{dx}{x} = \left[\ln(x^2 + 1) - \ln x\right] \cdot \frac{x}{x^2 + 1} \, dx
   \]
   This splits into two integrals:
   \[
   I = I_1 - I_2
   \]
   where
   \[
   I_1 = \int_0^1 \frac{x \ln(x^2 + 1)}{x^2 + 1} \, dx \quad \text{and} \quad I_2 = \int_0^1 \frac{x \ln x}{x^2 + 1} \, dx
   \]

2. **Compute \(I_1\)**:
   Use substitution \(u = \ln(x^2 + 1)\), \(du = \frac{2x}{x^2 + 1} \, dx\):
   \[
   I_1 = \frac{1}{2} \int_0^{\ln 2} u \, du = \frac{1}{2} \left[ \frac{u^2}{2} \right]_0^{\ln 2} = \frac{(\ln 2)^2}{4}
   \]

3. **Compute \(I_2\) using Integration by Parts**:
   Let \(u = \ln x\) and \(dv = \frac{x}{x^2 + 1} \, dx\). Then \(du = \frac{1}{x} \, dx\) and \(v = \frac{1}{2} \ln(x^2 + 1)\):
   \[
   I_2 = \left[ \frac{\ln x \cdot \ln(x^2 + 1)}{2} \right]_0^1 - \frac{1}{2} \int_0^1 \frac{\ln(x^2 + 1)}{x} \, dx
   \]
   The boundary term is zero. The remaining integral \(J = \int_0^1 \frac{\ln(x^2 + 1)}{x} \, dx\) is evaluated using a series expansion:
   \[
   J = \frac{\pi^2}{24}
   \]
   Thus,
   \[
   I_2 = -\frac{1}{2} \cdot \frac{\pi^2}{24} = -\frac{\pi^2}{48}
   \]

4. **Combine Results**:
   \[
   I = I_1 - I_2 = \frac{(\ln 2)^2}{4} + \frac{\pi^2}{48}
   \]

5. **Numerical Approximation**:
   Calculate the numerical value:
   \[
   \frac{(\ln 2)^2}{4} \approx 0.1201132535 \quad \text{and} \quad \frac{\pi^2}{48} \approx 0.2056167584
   \]
   Summing these gives:
   \[
   0.3257300118
   \]

### Final Answer
{"answer": "{\\frac{(\\ln 2)^2}{4} + \\frac{\\pi^2}{48}}", "numerical_answer": "0.3257300118"}