To solve the definite integral 

\[
\int\limits_{0}^{2}\frac{x^{-1/2}(2-x)^{-1/2}}{\sqrt{1+1 \times x(2-x)}}T_{3}\left(\sqrt{1+1 \times x(2-x)}\right)dx,
\]

where \( T_3 \) is the Chebyshev polynomial of the first kind of degree 3, we proceed with the following steps:

### Step 1: Simplify the Integrand

First, observe the expression inside the square root:

\[
1 + x(2 - x) = 1 + 2x - x^2 = 2 - (x^2 - 2x + 1) = 2 - (x - 1)^2.
\]

Let’s make a substitution to simplify the integral. Let:

\[
u = \sqrt{1 + x(2 - x)} = \sqrt{2 - (x - 1)^2}.
\]

Then, the derivative of \( u \) with respect to \( x \) is:

\[
\frac{du}{dx} = \frac{-2(x - 1)}{2\sqrt{2 - (x - 1)^2}} = \frac{-(x - 1)}{u}.
\]

However, this substitution seems complicated. Instead, let’s consider a trigonometric substitution.

### Step 2: Trigonometric Substitution

Let:

\[
x = 1 + \sin \theta, \quad \text{where } \theta \in \left[-\frac{\pi}{2}, \frac{\pi}{2}\right].
\]

Then:

\[
dx = \cos \theta \, d\theta,
\]

and the limits transform as follows:

- When \( x = 0 \), \( 1 + \sin \theta = 0 \) implies \( \sin \theta = -1 \), so \( \theta = -\frac{\pi}{2} \).
- When \( x = 2 \), \( 1 + \sin \theta = 2 \) implies \( \sin \theta = 1 \), so \( \theta = \frac{\pi}{2} \).

Now, express the integrand in terms of \( \theta \):

\[
x^{-1/2} = (1 + \sin \theta)^{-1/2}, \quad (2 - x)^{-1/2} = (1 - \sin \theta)^{-1/2},
\]

\[
\sqrt{1 + x(2 - x)} = \sqrt{2 - (x - 1)^2} = \sqrt{2 - \sin^2 \theta} = \sqrt{1 + \cos^2 \theta},
\]

since \( 2 - \sin^2 \theta = 1 + \cos^2 \theta \).

The Chebyshev polynomial \( T_3(u) \) is given by:

\[
T_3(u) = 4u^3 - 3u.
\]

Thus, the integrand becomes:

\[
\frac{(1 + \sin \theta)^{-1/2}(1 - \sin \theta)^{-1/2}}{\sqrt{1 + \cos^2 \theta}} T_3\left(\sqrt{1 + \cos^2 \theta}\right) \cos \theta.
\]

Simplify the product \( (1 + \sin \theta)^{-1/2}(1 - \sin \theta)^{-1/2} \):

\[
(1 - \sin^2 \theta)^{-1/2} = (\cos^2 \theta)^{-1/2} = \frac{1}{|\cos \theta|}.
\]

Since \( \theta \in \left[-\frac{\pi}{2}, \frac{\pi}{2}\right] \), \( \cos \theta \geq 0 \), so \( |\cos \theta| = \cos \theta \). Therefore, the integrand simplifies to:

\[
\frac{1}{\cos \theta} \cdot \frac{1}{\sqrt{1 + \cos^2 \theta}} \cdot \left(4(1 + \cos^2 \theta)^{3/2} - 3\sqrt{1 + \cos^2 \theta}\right) \cdot \cos \theta.
\]

The \( \cos \theta \) terms cancel out:

\[
\frac{4(1 + \cos^2 \theta)^{3/2} - 3\sqrt{1 + \cos^2 \theta}}{\sqrt{1 + \cos^2 \theta}} = 4(1 + \cos^2 \theta) - 3 = 4 \cos^2 \theta + 1.
\]

Thus, the integral becomes:

\[
\int_{-\pi/2}^{\pi/2} (4 \cos^2 \theta + 1) d\theta.
\]

### Step 3: Evaluate the Simplified Integral

Now, compute:

\[
\int_{-\pi/2}^{\pi/2} (4 \cos^2 \theta + 1) d\theta.
\]

Using the identity \( \cos^2 \theta = \frac{1 + \cos 2\theta}{2} \):

\[
4 \cos^2 \theta + 1 = 4 \left(\frac{1 + \cos 2\theta}{2}\right) + 1 = 2 + 2 \cos 2\theta + 1 = 3 + 2 \cos 2\theta.
\]

Thus, the integral is:

\[
\int_{-\pi/2}^{\pi/2} (3 + 2 \cos 2\theta) d\theta = 3 \pi + 2 \left[\frac{\sin 2\theta}{2}\right]_{-\pi/2}^{\pi/2} = 3 \pi + \left[\sin 2\theta\right]_{-\pi/2}^{\pi/2} = 3 \pi + 0 = 3 \pi.
\]

### Step 4: Numerical Approximation

The exact value of the integral is \( 3\pi \). A numerical approximation to 10 decimal places is:

\[
3\pi \approx 9.4247779608.
\]

### Final Answer

```json
{"answer": "3\\pi", "numerical_answer": "9.4247779608"}
```