<think>
Okay, let's see. I need to compute the definite integral from 0 to 2.0 of x^(1/2) times (2.0 - x)^(-1/2) times cos(1.0 times sqrt(x(2.0 - x))) dx. Hmm, that looks a bit complicated. Let me break it down step by step.

First, the integrand is x^(1/2) * (2 - x)^(-1/2) * cos(sqrt(x(2 - x))). The limits are from 0 to 2. Maybe a substitution would help here. The expression under the square root in the cosine is x(2 - x). Let me consider a substitution that simplifies that part.

Let me try substituting t = x - 1. That might center the interval around 0. But when x goes from 0 to 2, t goes from -1 to 1. Then x = t + 1, dx = dt. The expression x(2 - x) becomes (t + 1)(1 - t) = 1 - t^2. So sqrt(x(2 - x)) becomes sqrt(1 - t^2). That's a good sign because sqrt(1 - t^2) is a standard form, maybe leading to trigonometric substitution.

But let's see. The integrand becomes (t + 1)^(1/2) * (1 - t)^(-1/2) * cos(sqrt(1 - t^2)) * dt. Hmm, not sure if that's better. Alternatively, maybe another substitution.

Wait, let's consider a trigonometric substitution. Since we have sqrt(x(2 - x)), which is similar to sqrt(a^2 - (x - a)^2) if a is 1. Wait, x(2 - x) = 2x - x^2 = -(x^2 - 2x) = -(x^2 - 2x +1 -1) = -(x -1)^2 +1. So it's 1 - (x -1)^2. So sqrt(x(2 -x)) = sqrt(1 - (x -1)^2). That's like the equation of a circle. So maybe substituting x -1 = sinθ. Let's try that.

Let me set θ such that x -1 = sinθ. Then dx = cosθ dθ. When x = 0, sinθ = -1, so θ = -π/2. When x = 2, sinθ = 1, so θ = π/2. The limits become from -π/2 to π/2. Let's substitute.

x = 1 + sinθ, so 2 - x = 1 - sinθ. Then sqrt(x(2 -x)) = sqrt((1 + sinθ)(1 - sinθ)) = sqrt(1 - sin²θ) = cosθ. So the cosine term becomes cos(1.0 * cosθ) = cos(cosθ).

Now, the integrand:

x^(1/2) = (1 + sinθ)^(1/2)

(2 - x)^(-1/2) = (1 - sinθ)^(-1/2)

Multiply those together: (1 + sinθ)^(1/2) / (1 - sinθ)^(1/2) = sqrt[(1 + sinθ)/(1 - sinθ)]

Multiply numerator and denominator by (1 + sinθ):

sqrt[(1 + sinθ)^2 / (1 - sin²θ)] = sqrt[(1 + sinθ)^2 / cos²θ] = (1 + sinθ)/cosθ

So the integrand becomes (1 + sinθ)/cosθ * cos(cosθ) * dx. But dx = cosθ dθ. So substituting all together:

Integral from θ = -π/2 to π/2 of [ (1 + sinθ)/cosθ * cos(cosθ) * cosθ dθ ]

The cosθ in the denominator cancels with the cosθ from dx. So we have:

Integral from -π/2 to π/2 of (1 + sinθ) * cos(cosθ) dθ

Hmm, that's better. Now, split the integral into two parts:

Integral of cos(cosθ) dθ + Integral of sinθ * cos(cosθ) dθ, both from -π/2 to π/2.

Let's consider the first integral: Integral of cos(cosθ) dθ from -π/2 to π/2. The function cos(cosθ) is even because cos(cos(-θ)) = cos(cosθ). So we can write 2 * Integral from 0 to π/2 of cos(cosθ) dθ.

The second integral: Integral of sinθ * cos(cosθ) dθ from -π/2 to π/2. The integrand is an odd function because sin(-θ) * cos(cos(-θ)) = -sinθ * cos(cosθ). Therefore, the integral over a symmetric interval around zero is zero.

So the entire integral is 2 * Integral from 0 to π/2 of cos(cosθ) dθ + 0.

Therefore, the original integral simplifies to 2 * ∫₀^{π/2} cos(cosθ) dθ.

Now, the integral ∫ cos(cosθ) dθ from 0 to π/2 is a known integral and relates to the Bessel functions. Specifically, the integral of cos(a cosθ) dθ from 0 to π is π J_0(a), where J_0 is the Bessel function of the first kind of order zero. But our integral is from 0 to π/2, not π. Wait, let me check.

Wait, the standard integral is ∫₀^π cos(a cosθ) dθ = π J_0(a). So if we have ∫₀^{π/2} cos(cosθ) dθ, it's half of that? Not exactly. Let me verify.

Actually, the integral from 0 to π/2 of cos(a cosθ) dθ is (π/2) [J_0(a) + something]? Wait, maybe not. Let me recall the integral representation of Bessel functions. The Bessel function J_n(x) can be represented as (1/π) ∫₀^π cos(nθ - x sinθ) dθ. For n=0, J_0(x) = (1/π) ∫₀^π cos(x sinθ) dθ. But our integral is cos(a cosθ). Hmm, maybe another substitution.

Alternatively, perhaps express cos(cosθ) in terms of a series expansion. Let's consider expanding cos(z) where z = cosθ. The Taylor series for cos(z) is Σ (-1)^k z^{2k}/(2k)!.

So cos(cosθ) = Σ_{k=0}^∞ (-1)^k (cosθ)^{2k}/(2k)! = Σ (-1)^k cos^{2k}θ/(2k)!.

But integrating term by term: ∫₀^{π/2} cos^{2k}θ dθ. The integral is known; it's (π/2) * (2k)! / (2^{2k} (k!)^2). So putting it all together:

∫₀^{π/2} cos(cosθ) dθ = Σ_{k=0}^∞ (-1)^k/(2k)! * (π/2) * (2k)! / (2^{2k} (k!)^2) ) = (π/2) Σ_{k=0}^∞ (-1)^k / (2^{2k} (k!)^2 )

But this series is actually (π/2) J_0(1), because J_0(x) = Σ_{k=0}^∞ (-1)^k (x/2)^{2k} / (k!)^2. So when x=1, J_0(1) = Σ (-1)^k (1/2)^{2k} / (k!)^2. Therefore, the integral ∫₀^{π/2} cos(cosθ) dθ = (π/2) J_0(1).

Wait, but the standard integral is ∫₀^π cos(x cosθ) dθ = π J_0(x). So if we take x=1, then ∫₀^π cos(cosθ) dθ = π J_0(1). Therefore, ∫₀^{π/2} cos(cosθ) dθ would be half of that? Not exactly, because the integral from 0 to π/2 is not half of the integral from 0 to π. Let me check.

Wait, the function cos(cosθ) is symmetric around θ=π/2. Because cos(cos(π - θ)) = cos(cos(π - θ)) = cos(-cosθ) = cos(cosθ), since cosine is even. Wait, cos(π - θ) = -cosθ, so cos(cos(π - θ)) = cos(-cosθ) = cos(cosθ). So the function is symmetric around θ=π/2. Therefore, the integral from 0 to π/2 is equal to the integral from π/2 to π. Therefore, ∫₀^{π} cos(cosθ) dθ = 2 ∫₀^{π/2} cos(cosθ) dθ. Therefore, ∫₀^{π/2} cos(cosθ) dθ = (π/2) J_0(1).

Therefore, the original integral is 2 * (π/2) J_0(1) = π J_0(1). So the exact answer is π times the Bessel function of the first kind of order zero evaluated at 1.

So the exact answer is π J_0(1). Now, the problem says to compute the integral analytically. But Bessel functions are considered special functions, so maybe that's the analytical form. Alternatively, is there a way to express this integral in terms of elementary functions? I don't think so. The presence of cos(sqrt(x(2 -x))) suggests that it's not an elementary integral, so the answer is in terms of the Bessel function.

Therefore, the exact answer is π J_0(1). Now, for the numerical approximation. J_0(1) is a known value. Let me recall that J_0(1) ≈ 0.7651976866. So π times that is approximately 3.1415926536 * 0.7651976866 ≈ let's compute that.

First, 0.7651976866 * 3 = 2.2955930598

0.7651976866 * 0.1415926536 ≈ 0.7651976866 * 0.1 = 0.07651976866

0.7651976866 * 0.0415926536 ≈ approx 0.7651976866 * 0.04 = 0.0306079075

0.7651976866 * 0.0015926536 ≈ approx 0.001218

Adding those: 0.07651976866 + 0.0306079075 = 0.10712767616 + 0.001218 ≈ 0.10834567616

Total: 2.2955930598 + 0.10834567616 ≈ 2.40393873596

But let me use a calculator for more precision. Alternatively, look up J_0(1):

J_0(1) ≈ 0.7651976865579665514497 (from tables or calculator)

So π * J_0(1) ≈ 3.141592653589793 * 0.7651976865579666 ≈

Let me compute this:

3.141592653589793 * 0.7651976865579666

First, multiply 3 * 0.7651976865579666 = 2.2955930596739

0.141592653589793 * 0.7651976865579666 ≈

0.1 * 0.7651976865579666 = 0.07651976865579666

0.041592653589793 * 0.7651976865579666 ≈

Compute 0.04 * 0.7651976865579666 = 0.030607907462318664

0.001592653589793 * 0.7651976865579666 ≈ approx 0.001218

Adding these parts: 0.07651976865579666 + 0.030607907462318664 = 0.10712767611811532 + 0.001218 ≈ 0.10834567611811532

Total: 2.2955930596739 + 0.10834567611811532 ≈ 2.4039387357920153

But let's check with a calculator. Alternatively, use more precise multiplication:

0.141592653589793 * 0.7651976865579666

Break it down:

0.1 * 0.7651976865579666 = 0.07651976865579666

0.04 * 0.7651976865579666 = 0.030607907462318664

0.001592653589793 * 0.7651976865579666 ≈

First, 0.001 * 0.7651976865579666 = 0.0007651976865579666

0.000592653589793 * 0.7651976865579666 ≈

Approximate 0.0005 * 0.7651976865579666 = 0.0003825988432789833

0.000092653589793 * 0.7651976865579666 ≈ ~0.0000709

Adding these: 0.0007651976865579666 + 0.0003825988432789833 = 0.0011477965298369499 + 0.0000709 ≈ 0.00121869652983695

So total for 0.141592653589793 * 0.7651976865579666 is 0.07651976865579666 + 0.030607907462318664 + 0.00121869652983695 ≈ 0.10834637264795227

Adding to the 3 * part: 2.2955930596739 + 0.10834637264795227 ≈ 2.4039394323218523

So π J_0(1) ≈ 2.4039394323218523. Let me check with a calculator. Alternatively, use a calculator for J_0(1):

J_0(1) ≈ 0.7651976865579666

Multiply by π: 0.7651976865579666 * π ≈ 2.4039394306344133

So approximately 2.4039394306. Rounded to 10 decimal places, that's 2.4039394306.

But let me confirm with a more precise calculation. Alternatively, use a computational tool. Since I don't have one here, but assuming that J_0(1) is approximately 0.7651976866, then π times that is approximately 3.1415926536 * 0.7651976866 ≈ 2.4039394306.

Therefore, the numerical approximation is approximately 2.4039394306.

So the exact answer is π J_0(1), and the numerical approximation is approximately 2.4039394306.

Therefore, the final answer should be:

Exact answer: \pi J_0(1)

But the problem says to present the exact answer in LaTeX. Since J_0 is a standard function, it's acceptable. So the exact answer is π J₀(1), which in LaTeX is \pi J_0(1).

But wait, the problem says "compute the integral analytically to obtain the exact answer". If the answer is in terms of a Bessel function, that's acceptable as an exact answer. So yes, the exact answer is π J₀(1), and the numerical value is approximately 2.4039394306.
</think>

{"answer": "\\pi J_0(1)", "numerical_answer": "2.4039394306"}