Let’s compute
\[
I = \int_0^1 \frac{\ln(x + x^{-1})}{x + x^{-1}}\,dx.
\]

### Step 1: Substitution

Let’s substitute \( x = e^{-y} \). Then:
- As \( x \to 0^+ \), \( y \to +\infty \).
- As \( x \to 1 \), \( y \to 0 \).
- \( dx = -e^{-y} dy = -x\,dy \).

Now, compute \( x + x^{-1} = e^{-y} + e^{y} = 2 \cosh y \).

So,
\[
\ln(x + x^{-1}) = \ln(2 \cosh y), \qquad x + x^{-1} = 2\cosh y
\]

Write the integral:
\[
I = \int_{+\infty}^0 \frac{\ln(2 \cosh y)}{2\cosh y} (-e^{-y} dy)
\]
\[
= \int_0^{+\infty} \frac{\ln(2 \cosh y)}{2\cosh y} e^{-y} dy
\]

But \( e^{-y} \) in the numerator. Let's keep track of that.

So,
\[
I = \int_{0}^{\infty} \frac{\ln(2 \cosh y)}{2\cosh y}\, e^{-y} dy
\]

Now, \( 2\cosh y = e^y + e^{-y} \), and \( e^{-y}/(2\cosh y) = 1/(e^{y} + e^{-y}) \).

Thus:
\[
I = \int_0^\infty \frac{\ln(2 \cosh y)}{e^y + e^{-y}} dy
\]

But \( e^y + e^{-y} = 2\cosh y \), so we get:
\[
I = \int_0^\infty \frac{\ln(2\cosh y)}{2\cosh y} dy
\]

Wait: this is exactly the same form as before! That is, the substitution cycles back to itself.

Let’s try another approach.

---

### Step 2: Symmetrization

Let’s try substituting \( x \to 1/x \):

For the original integral:
\[
I = \int_0^1 \frac{\ln(x + x^{-1})}{x + x^{-1}} dx
\]
Substitute \( x = 1/t \), \( dx = -dt/t^2 \), when \( x: 0\to 1 \), \( t: \infty \to 1 \):

\[
I = \int_{\infty}^1 \frac{\ln((1/t) + t)}{(1/t) + t} \cdot \left(-\frac{dt}{t^2}\right)
\]
\[
= \int_1^{\infty} \frac{\ln(t + 1/t)}{t + 1/t} \cdot \frac{dt}{t^2}
\]

But \( t + 1/t \) is symmetric in \( t \) and \( 1/t \), and so is \( \ln(t + 1/t) \). Let's write:

\[
I = \int_1^{\infty} \frac{\ln(t + 1/t)}{t^2 (t + 1/t)} dt
\]
Now, add this to original \( I \):

\[
I' = \int_0^1 \frac{\ln(x + x^{-1})}{x + x^{-1}} dx + \int_1^{\infty} \frac{\ln(x + x^{-1})}{x^2 (x + x^{-1})} dx
\]
\[
= \int_0^{\infty} \frac{\ln(x + x^{-1})}{x^2 (x + x^{-1})} \cdot \left[x^2 \mathbf{1}_{0<x<1} + \mathbf{1}_{x>1}\right] dx
\]
But this seems less helpful.

---

### Step 3: Series Expansion

Let’s find a series for \( \frac{\ln(x + x^{-1})}{x + x^{-1}} \) valid for \( 0 < x < 1 \).

Let’s use \( x + x^{-1} = 2\cosh y \), \( x = e^{-y}, y>0 \), and express \( \ln(2\cosh y) \).

Recall the expansion:
\[
\ln(2\cosh y) = \ln 2 + \sum_{k=1}^{\infty} \frac{(-1)^{k+1}}{k} \frac{e^{-2ky}}{1}
\]
But perhaps more useful:

From the integral
\[
I = \int_0^1 \frac{\ln(x + x^{-1})}{x + x^{-1}} dx
\]
Let’s try expanding the numerator.

*Let’s try expressing the denominator in terms of a series:*

\( x + x^{-1} = x + 1/x \), so for \( 0 < x < 1 \):

\[
\frac{1}{x + x^{-1}} = \frac{1}{x + x^{-1}} = \frac{x}{x^2 + 1}
\]

Let’s check:
\[
x + x^{-1} = \frac{x^2 + 1}{x} \implies \frac{1}{x + x^{-1}} = \frac{x}{x^2 + 1}
\]
So the integral becomes
\[
I = \int_0^1 \ln(x + x^{-1}) \cdot \frac{x}{x^2 + 1} dx
\]

*This is a much friendlier form!*

---

### Step 4: Further Simplification

Let’s write \( \ln(x + x^{-1}) \), but recall \( x + x^{-1} = \frac{x^2 + 1}{x} \), so

\[
\ln(x + x^{-1}) = \ln(x^2 + 1) - \ln x
\]

So
\[
I = \int_0^1 \frac{x}{x^2 + 1} \left( \ln(x^2 + 1) - \ln x \right) dx
\]
\[
= \int_0^1 \frac{x \ln(x^2 + 1)}{x^2 + 1} dx - \int_0^1 \frac{x \ln x}{x^2 + 1} dx
\]
Call
\[
I_1 = \int_0^1 \frac{x \ln(x^2 + 1)}{x^2 + 1} dx,\quad
I_2 = \int_0^1 \frac{x \ln x}{x^2 + 1} dx
\]

So,
\[
I = I_1 - I_2
\]

---

#### Evaluate \(I_1\):

Let \( u = x^2 + 1 \implies du = 2x dx \implies x dx = \frac12 du \)

When \( x = 0, u = 1 \), when \( x = 1, u = 2 \)

So,
\[
I_1 = \int_0^1 \frac{x \ln(x^2 + 1)}{x^2 + 1} dx = \frac12 \int_{1}^{2} \frac{\ln u}{u} du = \frac12 \left. \frac12 \ln^2 u \right|_{u=1}^{u=2} = \frac14 \left( (\ln 2)^2 - (\ln 1)^2 \right)
\]
\[
= \frac14 (\ln 2)^2
\]

---

#### Evaluate \(I_2\):

\[
I_2 = \int_0^1 \frac{x\ln x}{x^2 + 1} dx
\]
Let’s use substitution \( u = x^2 \implies x = \sqrt u, dx = \frac{du}{2\sqrt u} \)

Alternatively, integrate by parts:

Let’s put \( u = \ln x \), \( dv = \frac{x}{x^2 + 1} dx \)
- \( du = \frac{1}{x} dx \)
- \( v = \frac12 \ln(x^2 + 1) \) (since \( \frac{d}{dx} \ln(x^2+1) = \frac{2x}{x^2+1} \))

Thus,
\[
I_2 = u v \Big|_0^1 - \int_0^1 v du
\]
\( u = \ln x \to -\infty \) as \( x \to 0 \), but \( x\ln x \to 0 \) as \( x \to 0 \), perhaps OK.

Let’s check the first term:

At \( x=1 \), \( u=0, v = \frac12 \ln 2 \), the product is 0.
At \( x=0 \), \( u \to -\infty \), \( v \to \frac12 \ln 1 = 0 \), product is 0.

So,
\[
I_2 = - \int_0^1 \frac12 \ln(x^2+1) \cdot \frac{1}{x} dx
\]
\[
= -\frac12 \int_0^1 \frac{\ln(x^2+1)}{x} dx
\]

Let’s let \( t = x^2 \implies x = \sqrt t, dx = \frac{dt}{2\sqrt t} \)
When \( x = 0, t = 0 \) ; \( x=1, t=1 \):

\[
\int_0^1 \frac{\ln(x^2+1)}{x} dx =
\int_{x=0}^{1} \frac{\ln(x^2+1)}{x} dx = \int_{t=0}^{1} \frac{\ln(t+1)}{\sqrt t} \cdot \frac{dt}{2\sqrt t}
= \frac12 \int_0^1 \frac{\ln(t+1)}{t} dt
\]
But that's not quite right (since \( 1/x \, dx \) relates to \( 1/t \, dt \)).

Alternatively, let’s just let \( x = e^{-u}, u: 0 \to \infty \):

When \( x=0, u=\infty \); \( x=1, u=0 \).
\( dx = -e^{-u} du = -x du \)
So,

\[
I_2 = \int_0^1 \frac{x\ln x}{x^2 + 1} dx 
= \int_{u = \infty}^{0} \frac{e^{-u}(-u)}{e^{-2u} + 1} (-e^{-u} du)
= \int_0^{\infty} \frac{u e^{-2u}}{1 + e^{-2u}} du
\]
Let’s double-check:

- \( x = e^{-u} \implies x \ln x = -u e^{-u} \), \( x^2 + 1 = e^{-2u} + 1 \)
- \( dx = -e^{-u} du \)
Thus, \( x \ln x \, dx = -u e^{-u} \cdot (-e^{-u} du) = u e^{-2u} du \)
So,

\[
I_2 = \int_0^\infty \frac{u e^{-2u}}{1 + e^{-2u}} du
\]
Note:
\[
\frac{e^{-2u}}{1+e^{-2u}} = \sum_{k=1}^\infty (-1)^{k+1} e^{-2ku}
\]
Therefore,

\[
I_2 = \int_0^{\infty} u \sum_{k=1}^{\infty} (-1)^{k+1} e^{-2ku} du = \sum_{k=1}^{\infty} (-1)^{k+1} \int_0^{\infty} u e^{-2k u} du
\]
But
\[
\int_0^{\infty} u e^{-a u} du = \frac{1}{a^2}
\]
Thus,
\[
I_2 = \sum_{k=1}^{\infty} (-1)^{k+1} \cdot \frac{1}{(2k)^2} = \frac{1}{4} \sum_{k=1}^{\infty} \frac{(-1)^{k+1}}{k^2}
\]

But
\[
\sum_{k=1}^{\infty} \frac{(-1)^{k+1}}{k^2} = \eta(2)
\]
where \( \eta(s) = (1 - 2^{1-s}) \zeta(s) \) is the Dirichlet eta function.

For \( s=2 \):
\[
\eta(2) = (1 - 2^{-1}) \zeta(2) = \frac12 \zeta(2) = \frac{\pi^2}{12}
\]

Thus,
\[
I_2 = \frac{1}{4} \cdot \frac{\pi^2}{12} = \frac{\pi^2}{48}
\]

---

### Final Step: Assemble the Pieces

Recall:

- \( I_1 = \frac14 (\ln 2)^2 \)
- \( I_2 = \frac{\pi^2}{48} \)

So,
\[
I = I_1 - I_2 = \frac14 (\ln 2)^2 - \frac{\pi^2}{48}
\]

---

### Step 3: Numerical Evaluation

- \( \ln 2 \approx 0.69314718056 \)
- \( (\ln 2)^2 \approx 0.48089834696 \)
- \( \frac14 (\ln 2)^2 \approx 0.12022458674 \)
- \( \pi^2 \approx 9.86960440109 \)
- \( \frac{\pi^2}{48} \approx 0.20561259169 \)
- \( I \approx 0.12022458674 - 0.20561259169 = -0.08538800495 \)

Rounded to 10 decimal places:
\[
I \approx -0.0853880050
\]

---

### Final JSON

```json
{"answer": "\\frac{1}{4} (\\ln 2)^2 - \\frac{\\pi^2}{48}", "numerical_answer": "-0.0853880050"}
```