We start with the observation that for any real number t the identity

  ∫₀¹ (xᵗ – 1)/ln x dx = ln(t + 1)

holds. (This result can be verified by differentiating with respect to t under the integral sign.)

Now, write the given integral as a difference of two integrals:
  I = ∫₀¹ (x²⁰²³ – x²³)/ln x dx
    = ∫₀¹ [(x²⁰²³ – 1) – (x²³ – 1)]/ln x dx
    = ∫₀¹ (x²⁰²³ – 1)/ln x dx – ∫₀¹ (x²³ – 1)/ln x dx.

Using the established formula with t = 2023 for the first integral and t = 23 for the second, we get:
  ∫₀¹ (x²⁰²³ – 1)/ln x dx = ln(2023 + 1) = ln 2024,
  ∫₀¹ (x²³ – 1)/ln x dx = ln(23 + 1)   = ln 24.

Thus, the value of the integral is:
  I = ln 2024 – ln 24 = ln(2024/24).

Notice that 2024/24 simplifies by dividing numerator and denominator by 8:
  2024 ÷ 8 = 253  and  24 ÷ 8 = 3,
so that
  2024/24 = 253/3.

Thus, the exact answer is:
  I = ln(253/3).

For the numerical approximation, we compute:
  253/3 ≈ 84.3333333333
  ln(84.3333333333) ≈ 4.4348177102   (to 10 decimal places).

{"answer": "\\ln\\frac{253}{3}", "numerical_answer": "4.4348177102"}