Let's compute the integral:
\[
I = \int_{0}^{1} \arcsin\left(0.5x\right) \arccos x \; dx
\]

**Step 1. Consider substitution and integration by parts.**

Let’s let
\[
u = \arcsin\left(0.5x\right), \quad dv = \arccos x \, dx
\]
However, integrating \(\arccos x\) with respect to \(x\) directly is challenging. Instead, let's instead swap the order:
Let
\[
u = \arccos x, \quad dv = \arcsin(0.5x) dx
\]
Then,
\[
du = -\frac{1}{\sqrt{1-x^2}} dx
\]
To compute \(v\), we need to integrate \(\arcsin(0.5x)\):
Let’s recall that
\[
\int \arcsin(ax) dx = x \arcsin(ax) + \frac{\sqrt{1-a^2x^2}}{a} + C
\]
Let’s check this (by differentiating). Actually, the correct formula is:
\[
\int \arcsin(ax) dx = x \arcsin(ax) + \frac{\sqrt{1-(ax)^2}}{a} + C
\]

Therefore,
\[
\int \arcsin(0.5x) dx = x \arcsin(0.5x) + 2\sqrt{1-0.25x^2} + C
\]

Now, apply integration by parts:
\[
I = \left. \arccos x \cdot \left[ x \arcsin(0.5x) + 2\sqrt{1-0.25x^2} \right] \right|_{x=0}^{x=1} - \int_{0}^{1} \left[ x \arcsin(0.5x) + 2\sqrt{1-0.25x^2} \right] \cdot \left( -\frac{1}{\sqrt{1-x^2}} \right) dx
\]
\[
= \left. \arccos x \cdot \left[ x \arcsin(0.5x) + 2\sqrt{1-0.25x^2} \right] \right|_{0}^{1} + \int_{0}^{1} \frac{ x \arcsin(0.5x) + 2\sqrt{1-0.25x^2} }{\sqrt{1-x^2}} dx
\]

Compute the boundary terms:

At \(x=1\):
\[
\arccos 1 = 0
\]
So the term vanishes.

At \(x=0\):
\[
\arccos 0 = \frac{\pi}{2}, \quad x \arcsin(0.5x) = 0, \quad 2\sqrt{1-0} = 2
\]
So,
\[
\arccos(0) \cdot [0 + 2] = \frac{\pi}{2} \cdot 2 = \pi
\]

So, the boundary term is:
\[
0 - \pi = -\pi
\]

So,
\[
I = -\pi + \int_{0}^{1} \frac{ x \arcsin(0.5x) + 2\sqrt{1-0.25x^2} }{\sqrt{1-x^2}} dx
\]
\[
= -\pi + \int_{0}^{1} \frac{x \arcsin(0.5x)}{\sqrt{1-x^2}} dx + 2 \int_{0}^{1} \frac{ \sqrt{1-0.25x^2} }{\sqrt{1-x^2}} dx
\]

Let’s denote:
\[
I_1 = \int_{0}^{1} \frac{x \arcsin(0.5x)}{\sqrt{1-x^2}} dx
\]
\[
I_2 = 2 \int_{0}^{1} \frac{ \sqrt{1-0.25x^2} }{\sqrt{1-x^2}} dx
\]

Let's tackle \(I_2\) first.

---

### \(I_2 = 2 \int_{0}^{1} \frac{ \sqrt{1-0.25x^2} }{\sqrt{1-x^2}} dx\)

Let’s use \(x = \sin \theta\), so that \(dx = \cos \theta d\theta\), \(x^2 = \sin^2 \theta\), as \(x\) goes from 0 to 1, \(\theta\) goes from 0 to \(\frac{\pi}{2}\).
Then,
\[
I_2 = 2 \int_{x=0}^{1} \frac{ \sqrt{1-0.25x^2} }{\sqrt{1-x^2}} dx = 2 \int_{\theta=0}^{\pi/2} \frac{ \sqrt{1 - 0.25 \sin^2 \theta} }{ \sqrt{1 - \sin^2 \theta} } \cos \theta d\theta
\]
But \(\sqrt{1 - \sin^2 \theta} = \cos \theta\), so
\[
I_2 = 2 \int_{0}^{\pi/2} \sqrt{1 - 0.25 \sin^2 \theta} d\theta
\]

Let’s write \(1 - 0.25 \sin^2 \theta = 1 - \frac{1}{4} \sin^2 \theta\).

This is a standard form of an elliptic integral:
\[
\int_{0}^{\pi/2} \sqrt{1 - k^2 \sin^2 \theta} d\theta = E(k)
\]
where \(E(k)\) is the complete elliptic integral of the second kind, and \(k = 1/2\).

Therefore,
\[
I_2 = 2 E\left( \frac{1}{2} \right )
\]

---

### \(I_1 = \int_{0}^{1} \frac{x\arcsin(0.5x)}{\sqrt{1-x^2}} dx\)

Again, substitute \(x = \sin \theta\):
When \(x=0\), \(\theta=0\); \(x=1\), \(\theta=\pi/2\).
\[
x = \sin \theta, \quad dx = \cos \theta d\theta, \quad \sqrt{1-x^2} = \cos \theta
\]
So,
\[
I_1 = \int_{x=0}^{1} \frac{ x \arcsin(0.5x) }{ \sqrt{1-x^2} } dx = \int_{0}^{\pi/2} \frac{ \sin \theta \arcsin(0.5 \sin \theta) }{ \cos \theta } \cos \theta d\theta
\]
The \(\cos \theta\) cancels:
\[
I_1 = \int_{0}^{\pi/2} \sin \theta \arcsin(0.5 \sin \theta) d\theta
\]

Let’s write
\[
I_1 = \int_{0}^{\pi/2} \sin \theta \arcsin\left( \frac{1}{2} \sin \theta \right ) d\theta
\]

Let’s make another substitution for the inner arcsin. Let's let
Let’s let \(u = \arcsin \left( \frac{1}{2} \sin \theta \right )\).
Then, 
\[
\sin u = \frac{1}{2}\sin \theta \implies \sin \theta = 2 \sin u
\]
We need to find \(d\theta\) in terms of \(du\).

But perhaps an alternative approach is to integrate by parts.

Let \(f(\theta) = \arcsin\left(\frac{1}{2} \sin \theta \right)\)
Let’s let 
\[
u = \arcsin\left(\frac{1}{2} \sin \theta \right), \quad dv = \sin \theta d\theta
\]
So,
\[
du = \frac{1/2 \cos\theta}{\sqrt{1 - (1/4) \sin^2\theta }} d\theta = \frac{ \cos \theta }{ 2 \sqrt{ 1 - (1/4)\sin^2\theta } } d\theta
\]
\[
v = -\cos \theta
\]

Therefore, integration by parts gives:
\[
I_1 = \left. -\cos\theta \cdot \arcsin\left( \frac{1}{2} \sin\theta \right ) \right|_{ 0 }^{ \pi/2 } + \int_{ 0 }^{ \pi/2 } \cos\theta \cdot \frac{ \cos \theta }{ 2 \sqrt{ 1 - \frac{1}{4} \sin^2\theta } } d\theta
\]
\[
= \left. -\cos\theta \cdot \arcsin\left( \frac{1}{2} \sin\theta \right ) \right|_{ 0 }^{ \pi/2 } + \frac{1}{2} \int_{0}^{\pi/2} \frac{ \cos^2 \theta }{ \sqrt{ 1 - \frac{1}{4} \sin^2\theta } } d\theta
\]

Evaluate the boundary term:
At \(\theta=0\), \(\cos\theta = 1\), \(\sin\theta = 0 \implies \arcsin( 0 ) = 0\), so \( -1 \cdot 0 = 0 \).
At \(\theta=\pi/2\), \(\cos(\pi/2) = 0\), so boundary term is zero.
Thus, boundary term vanishes.

So,
\[
I_1 = \frac{1}{2} \int_{0}^{\pi/2} \frac{ \cos^2 \theta }{ \sqrt{ 1 - \frac{1}{4} \sin^2\theta } } d\theta
\]

Recall,
\[
\cos^2 \theta = 1 - \sin^2\theta
\]
Thus,
\[
I_1 = \frac{1}{2} \left( \int_{0}^{\pi/2} \frac{ d\theta }{ \sqrt{ 1 - \frac{1}{4} \sin^2\theta } } - \int_{0}^{\pi/2} \frac{ \sin^2\theta d\theta }{ \sqrt{ 1 - \frac{1}{4} \sin^2\theta } } \right )
\]

The first integral is the complete elliptic integral of the first kind:
\[
K(k) = \int_{0}^{\pi/2} \frac{ d\theta }{ \sqrt{ 1 - k^2 \sin^2\theta } }
\]

So with \(k = 1/2\):
\[
K\left( \frac{1}{2} \right ) = \int_{0}^{\pi/2} \frac{ d\theta }{ \sqrt{ 1 - \frac{1}{4} \sin^2\theta } }
\]

The second integral:
\[
J = \int_{0}^{\pi/2} \frac{ \sin^2\theta d\theta }{ \sqrt{ 1 - \frac{1}{4} \sin^2\theta } }
\]

But
\[
\sin^2 \theta = 1 - \cos^2 \theta
\]
But more helpfully, there is a reduction formula:

Let’s note that (see Gradshteyn & Ryzhik 3.147):

\[
\int_{0}^{\pi/2} \frac{ \sin^2 \theta d\theta }{ \sqrt{ 1 - k^2 \sin^2\theta } } = \frac{1}{k^2}[ E(k) - (1 - k^2) K(k) ]
\]
With \(k = 1/2\), \(k^2 = 1/4\):

\[
J = \frac{1}{1/4}\left[ E\left( \frac{1}{2} \right ) - \left(1 - \frac{1}{4}\right) K\left( \frac{1}{2} \right ) \right ]
= 4 \left[ E\left( \frac{1}{2} \right ) - \frac{3}{4} K\left( \frac{1}{2} \right ) \right ]
\]

Therefore,

\[
I_1 = \frac{1}{2} \left( K\left( \frac{1}{2} \right ) - 4\left[ E\left( \frac{1}{2} \right ) - \frac{3}{4} K\left( \frac{1}{2} \right ) \right ] \right )
\]
\[
= \frac{1}{2}\left( K\left( \frac{1}{2} \right ) - 4 E\left( \frac{1}{2} \right ) + 3 K\left( \frac{1}{2} \right ) \right )
\]
\[
= \frac{1}{2} \left( 4 K\left( \frac{1}{2} \right ) - 4 E\left( \frac{1}{2} \right ) \right )
= 2 K\left( \frac{1}{2} \right ) - 2 E\left( \frac{1}{2} \right )
\]

So

\[
I_1 = 2 K\left( \frac{1}{2} \right ) - 2 E\left( \frac{1}{2} \right )
\]

---

Therefore, substitute back:
\[
I = -\pi + I_1 + I_2 = -\pi + [2 K(1/2) - 2 E(1/2)] + [2 E(1/2)]
\]
\[
I = -\pi + 2 K\left(\frac{1}{2}\right )
\]

---

### Final exact answer:

\[
\boxed{
\int_{0}^{1} \arcsin\left(0.5x\right) \arccos x \, dx
= 2 K\left( \frac{1}{2} \right ) - \pi
}
\]

where \(K(k)\) is the complete elliptic integral of the first kind.

---

### Step 3: Numerical approximation

The complete elliptic integral of the first kind for \(k=1/2\):
\[
K\left(\frac{1}{2}\right) \approx 1.6857503548
\]

So
\[
I \approx 2 \times 1.6857503548 - \pi \approx 3.3715007096 - 3.1415926536 \approx 0.2299080560
\]

---

### Step 4: JSON output

```json
{"answer": "2K\\left(\\frac{1}{2}\\right)-\\pi", "numerical_answer": "0.2299080560"}
```