Let's solve the definite integral: 
\[
\int_{-1}^{0} 5(x^6 + x)^4 \, dx
\]

### Step 1: Substitution

Let’s use the substitution:
Let \( u = x^6 + x \).
Then,
\[
\frac{du}{dx} = 6x^5 + 1 \implies du = (6x^5 + 1) dx
\]

But our integrand only has \( dx \), so a direct substitution is inconvenient. Instead, let's expand \((x^6 + x)^4\).

### Step 2: Binomial Expansion

We expand \((x^6 + x)^4\) using the binomial theorem:
\[
(x^6 + x)^4 = \sum_{k=0}^4 \binom{4}{k} (x^6)^{4-k} (x)^k = \sum_{k=0}^4 \binom{4}{k} x^{6(4-k) + k}
\]
\[
= \sum_{k=0}^4 \binom{4}{k} x^{24-5k}
\]
So, 
\[
\int_{-1}^{0} 5(x^6 + x)^4 dx = 5 \int_{-1}^{0} \sum_{k=0}^4 \binom{4}{k} x^{24-5k} dx
\]
\[
= 5 \sum_{k=0}^4 \binom{4}{k} \int_{-1}^0 x^{24-5k} dx
\]
The integral of \( x^n \) from \(-1\) to \(0\) is:
\[
\int_{-1}^0 x^n dx = \left[ \frac{x^{n+1}}{n+1} \right]_{-1}^0 = 0 - \frac{(-1)^{n+1}}{n+1} = \frac{(-1)^{n+2}}{n+1}
\]

### Step 3: Compute Each Term

Let’s calculate for each \( k \) from 0 to 4:

- For \( k = 0 \): \(\binom{4}{0} = 1\), exponent \( 24-5*0 = 24 \).
- For \( k = 1 \): \(\binom{4}{1} = 4\), exponent \( 24-5*1 = 19 \).
- For \( k = 2 \): \(\binom{4}{2} = 6\), exponent \( 24-5*2 = 14 \).
- For \( k = 3 \): \(\binom{4}{3} = 4\), exponent \( 24-5*3 = 9 \).
- For \( k = 4 \): \(\binom{4}{4} = 1\), exponent \( 24-5*4 = 4 \).

So,
\[
5 \sum_{k=0}^4 \binom{4}{k} \frac{(-1)^{24-5k+2}}{24-5k+1}
\]

Let’s write out each term:

1. **\(k=0\):**
\[
\binom{4}{0} = 1, \quad n_0 = 24
\]
\[
\frac{(-1)^{24+2}}{25} = \frac{(-1)^{26}}{25} = \frac{1}{25}
\]

2. **\(k=1\):**
\[
\binom{4}{1} = 4, \quad n_1 = 19
\]
\[
\frac{(-1)^{21}}{20} = \frac{-1}{20}
\]

3. **\(k=2\):**
\[
\binom{4}{2} = 6, \quad n_2 = 14
\]
\[
\frac{(-1)^{16}}{15} = \frac{1}{15}
\]

4. **\(k=3\):**
\[
\binom{4}{3} = 4, \quad n_3 = 9
\]
\[
\frac{(-1)^{11}}{10} = \frac{-1}{10}
\]

5. **\(k=4\):**
\[
\binom{4}{4} = 1, \quad n_4 = 4
\]
\[
\frac{(-1)^6}{5} = \frac{1}{5}
\]

Plugging all in:
\[
5 \left( \frac{1}{25} \cdot 1 + 4 \cdot \left(-\frac{1}{20}\right) + 6 \cdot \frac{1}{15} + 4 \cdot \left(-\frac{1}{10}\right) + 1 \cdot \frac{1}{5} \right)
\]

\[
= 5 \left( \frac{1}{25} - \frac{4}{20} + \frac{6}{15} - \frac{4}{10} + \frac{1}{5} \right)
\]

\[
= 5 \left( \frac{1}{25} - \frac{1}{5} + \frac{2}{5} - \frac{2}{5} + \frac{1}{5} \right)
\]

Let’s compute each fraction:

\[
\frac{1}{25} - \frac{4}{20} + \frac{6}{15} - \frac{4}{10} + \frac{1}{5}
\]
Calculate each term numerically:

- \( \frac{1}{25} = 0.04 \)
- \( -\frac{4}{20} = -0.2 \)
- \( \frac{6}{15} = 0.4 \)
- \( -\frac{4}{10} = -0.4 \)
- \( \frac{1}{5} = 0.2 \)

Sum:

\( 0.04 - 0.2 + 0.4 - 0.4 + 0.2 = 0.04 + (-0.2 + 0.4) + (-0.4 + 0.2) = 0.04 + 0.2 - 0.2 = 0.04 \)

Now multiply by 5:

\[
5 \times 0.04 = 0.2
\]

### Step 4: Exact Form

Let’s write all as fractions:

\[
5 \left( \frac{1}{25} - \frac{4}{20} + \frac{6}{15} - \frac{4}{10} + \frac{1}{5} \right)
\]
Convert denominators to 300:

- \( \frac{1}{25} = \frac{12}{300} \)
- \( -\frac{4}{20} = -\frac{60}{300} \)
- \( \frac{6}{15} = \frac{120}{300} \)
- \( -\frac{4}{10} = -\frac{120}{300} \)
- \( \frac{1}{5} = \frac{60}{300} \)

Sum numerators:
\( 12 - 60 + 120 - 120 + 60 = 12 \)

So sum is \( \frac{12}{300} = \frac{1}{25} \)

Thus,
\[
5 \times \frac{1}{25} = \frac{1}{5}
\]

### Step 5: Numerical Approximation

\[
\frac{1}{5} = 0.2
\]

### Final JSON Output

```json
{"answer": "\\frac{1}{5}", "numerical_answer": "0.2000000000"}
```