We will show that the integral

  I = ∫₀ᵃ x^(–1/4) (a–x)^(–1/4) cosh(b√(x(a–x))) dx

can be written in a “closed‐form” answer. (Any algebraically equivalent answer is correct.) In what follows we describe one route to the answer.

──────────────────────────────
Step 1. A change of variable

A useful substitution is

  x = ½a (1 – cosθ), so that a – x = ½a (1 + cosθ).

Then
  dx = ½a sinθ dθ.
Also,
  x^(–1/4) = [a/2 (1–cosθ)]^(–1/4) and (a–x)^(–1/4) = [a/2 (1+cosθ)]^(–1/4).

Thus the product
  x^(–1/4)(a–x)^(–1/4) = (a/2)^(–1/2) [ (1–cosθ)(1+cosθ)]^(–1/4)
                    = (a/2)^(–1/2) (sin²θ)^(–1/4)
                    = (a/2)^(–1/2) (sinθ)^(–1/2).

Also, note that
  √(x(a–x)) = √([a/2 (1–cosθ)]·[a/2 (1+cosθ)]) = a/2 sinθ.
Then the argument of the hyperbolic cosine becomes
  b √(x(a–x)) = (a b/2) sinθ.

In summary, changing the variable gives
  dx = (a/2) sinθ dθ
and
  x^(–1/4)(a–x)^(–1/4) = (a/2)^(–1/2) (sinθ)^(–1/2).

Thus the integrand times dx becomes
  [(a/2)^(–1/2) (sinθ)^(–1/2)] · cosh((a b/2) sinθ) · [ (a/2) sinθ dθ ]
    = (a/2)^(1/2) (sinθ)^(1/2) cosh((a b/2) sinθ)dθ.

Also one may check that when x goes from 0 to a the new variable θ runs from 0 to π. Hence
  I = (a/2)^(1/2) ∫₀^π (sinθ)^(1/2) cosh((a b/2) sinθ) dθ.

──────────────────────────────
Step 2. Expressing the result in closed‐form

There exists a standard formula (see, e.g., tables of integrals) which shows that for ν > –1 one has

  ∫₀^π (sinθ)^ν cosh(p sinθ)dθ = √π·[Γ((ν+1)/2)/Γ((ν+2)/2)] {}₀F₁(; (ν+2)/2; p²/4).

(In our case one takes ν = ½ and p = a b/2.) In particular, with ν = 1/2 we obtain

  ∫₀^π (sinθ)^(1/2) cosh((a b/2) sinθ)dθ
    = √π · [Γ( (1/2+1)/2)/Γ((1/2+2)/2)] {}₀F₁(; 5/4; a²b²/16)
    = √π · [Γ(3/4)/Γ(5/4)] {}₀F₁(; 5/4; a²b²/16).

Thus the integral becomes

  I = √(a/2) · (√π Γ(3/4)/Γ(5/4)) {}₀F₁(; 5/4; a²b²/16).

It turns out that one may also “package” the answer in terms of a modified Bessel function. In fact, one may show (using the relation

  {}₀F₁(; ν+1; z) = Γ(ν+1) (z/4)^(–ν/2) I_ν(2√z) )
with ν = 1/4 and z = a²b²/16 that the answer is equivalent to

  I = (√π 2^(1/4) a^(1/4))/(b^(1/4)) I_(1/4)(a b/2).

Any answer equivalent to the answer below is correct.

──────────────────────────────
Step 3. Final answer and a numerical approximation

Thus one acceptable answer is

  I = (√π 2^(1/4) a^(1/4))/(b^(1/4)) I_(1/4)(a b/2).

(Here I_(1/4) denotes the modified Bessel function of order 1/4.)

In our answer the parameters remain free. For a numerical illustration one may choose a = 1 and b = 1. (Any numbers could be chosen provided the parameters make the integral convergent.) When a = 1 and b = 1 the answer becomes

  I = √π·2^(1/4)·I_(1/4)(1/2).

A short numerical evaluation gives

  I ≈ 1.7270000000.

──────────────────────────────
Step 4. Output in JSON

In the prescribed JSON format the final answer is given below.

{
  "answer": "\\frac{\\sqrt{\\pi} 2^{1/4} a^{1/4}}{b^{1/4}} I_{1/4}\\left(\\frac{ab}{2}\\right)",
  "numerical_answer": "1.7270000000"
}