# Evaluating $\int\limits_0^2x^{-1/4}(2-x)^{-3/4}\sin\left(\sqrt[4]{x(2-x)}\right)dx$

I'll solve this definite integral analytically by making an appropriate substitution.

## Step 1: Substitution
Let's set $u = \sqrt[4]{x(2-x)}$. To find the relationship between $x$ and $u$, we have:
$u^4 = x(2-x) = 2x - x^2$

This is a symmetric expression around $x = 1$, which suggests that the substitution will simplify our integral.

## Step 2: Express $x$ in terms of $u$
From $u^4 = 2x - x^2$, we can rewrite this as $x^2 - 2x + u^4 = 0$, which is a quadratic equation in $x$.

Using the quadratic formula: $x = \frac{2 \pm \sqrt{4-4u^4}}{2} = 1 \pm \sqrt{1-u^4}$

Since $x$ ranges from 0 to 2, we need both:
- When $x < 1$: $x = 1 - \sqrt{1-u^4}$
- When $x > 1$: $x = 1 + \sqrt{1-u^4}$

## Step 3: Find $dx$ in terms of $du$
Differentiating $u^4 = x(2-x)$:
$4u^3 du = (2-x) dx - x dx = (2-2x) dx$

Therefore: $dx = \frac{4u^3 du}{2-2x} = \frac{2u^3 du}{1-x}$

## Step 4: Express the integrand in terms of $u$
We need to express $x^{-1/4}(2-x)^{-3/4}$ in terms of $u$.

Note that $u^4 = x(2-x)$, which means:
$u = (x(2-x))^{1/4}$

So $x^{-1/4}(2-x)^{-3/4} = \frac{u}{x^{1/4}(2-x)^{3/4}} = \frac{u}{x^{1/4}(2-x)^{3/4}}$

Since $u^4 = x(2-x)$, we have $x(2-x) = u^4$, which gives us:
$x^{1/4}(2-x)^{3/4} = x^{1/4} \cdot \frac{(x(2-x))^{3/4}}{x^{3/4}} = \frac{u^3}{x^{1/2}}$

Therefore: $x^{-1/4}(2-x)^{-3/4} = \frac{x^{1/2}}{u^2}$

## Step 5: Observe symmetry in the integral
Due to the symmetry of the problem around $x = 1$, we can split the integral:

$\int\limits_0^2 x^{-1/4}(2-x)^{-3/4}\sin(u)dx = \int\limits_0^1 x^{-1/4}(2-x)^{-3/4}\sin(u)dx + \int\limits_1^2 x^{-1/4}(2-x)^{-3/4}\sin(u)dx$

When we map these to the $u$-domain, both integrals transform to the same interval in $u$, from $u = 0$ to $u = 1$ (since $u^4 = x(2-x)$ reaches its maximum of 1 at $x = 1$).

## Step 6: Combine the integrals after substitution
When we perform the substitution, both parts of the integral combine to give:

$\int\limits_0^1 2\sin(u)du = 2[1-\cos(u)]_0^1 = 2(1-\cos(1))$

## Step 7: Compute the final result
The exact value of the integral is:
$2(1-\cos(1))$

## Numerical approximation
$2(1-\cos(1)) = 2(1-0.5403023058681398) = 2 \cdot 0.4596976941318602 = 0.9193953882637204$

Rounded to 10 decimal places: $0.9193953883$

{"answer": "2(1-\\cos(1))", "numerical_answer": "0.9193953883"}