
To solve the definite integral \(\int_{0}^{2} x^{-1/2}(2-x)^{-1/2} \cosh\left(\sqrt{x(2-x)}\right) \, dx\), we proceed with the following steps:


### Step 1: Substitution to Simplify the Integrand
First, observe that the term \(x(2-x)\) inside the square root can be rewritten by completing the square:  
\(x(2-x) = 1 - (x-1)^2\).  

We use the trigonometric substitution \(x = 1 + \sin\theta\), which implies \(dx = \cos\theta \, d\theta\). When \(x = 0\), \(\theta = -\pi/2\); when \(x = 2\), \(\theta = \pi/2\).  

Under this substitution:  
- \(x(2-x) = (1+\sin\theta)(1-\sin\theta) = 1 - \sin^2\theta = \cos^2\theta\), so \(\sqrt{x(2-x)} = \cos\theta\) (since \(\cos\theta \geq 0\) for \(\theta \in [-\pi/2, \pi/2]\)).  
- \(x^{-1/2}(2-x)^{-1/2} = \left(\cos^2\theta\right)^{-1/2} = 1/\cos\theta\).  

The integrand simplifies to:  
\[
x^{-1/2}(2-x)^{-1/2} \cosh\left(\sqrt{x(2-x)}\right) \, dx = \frac{1}{\cos\theta} \cdot \cosh(\cos\theta) \cdot \cos\theta \, d\theta = \cosh(\cos\theta) \, d\theta.
\]  


### Step 2: Simplify the Integral Limits
The integral limits transform from \(x \in [0, 2]\) to \(\theta \in [-\pi/2, \pi/2]\). Thus, the integral becomes:  
\[
\int_{-\pi/2}^{\pi/2} \cosh(\cos\theta) \, d\theta.
\]  

Since \(\cosh(\cos\theta)\) is even in \(\theta\) (because \(\cos(-\theta) = \cos\theta\) and \(\cosh\) is even), we can rewrite the integral as:  
\[
2 \int_{0}^{\pi/2} \cosh(\cos\theta) \, d\theta.
\]  


### Step 3: Use Integral Representation of Modified Bessel Function
Recall the integral representation of the modified Bessel function of the first kind, \(I_0(z)\):  
\[
I_0(z) = \frac{1}{\pi} \int_{0}^{\pi} e^{z \cos\theta} \, d\theta.
\]  

We express \(\cosh(\cos\theta)\) as \(\frac{e^{\cos\theta} + e^{-\cos\theta}}{2}\). The integral then becomes:  
\[
\int_{-\pi/2}^{\pi/2} \cosh(\cos\theta) \, d\theta = \int_{-\pi/2}^{\pi/2} \frac{e^{\cos\theta} + e^{-\cos\theta}}{2} \, d\theta.
\]  

By symmetry, this simplifies to:  
\[
\int_{0}^{\pi} \cosh(\sin\phi) \, d\phi \quad (\text{via substitution } \phi = \theta + \pi/2).
\]  

Using the integral representation of \(I_0(z)\) with \(z = 1\), we find:  
\[
\int_{0}^{\pi} \cosh(\cos\theta) \, d\theta = \pi I_0(1).
\]  


### Step 4: Exact and Numerical Results
The exact value of the integral is \(\pi I_0(1)\), where \(I_0(1)\) is the modified Bessel function of the first kind of order 0 evaluated at 1.  

Numerically, \(I_0(1) \approx 1.26606587775\), so:  
\[
\pi I_0(1) \approx 3.14159265359 \times 1.26606587775 \approx 3.9774652128.
\]  


### Final Answer
{"answer": "\(\pi I_0(1)\)", "numerical_answer": "3.9774652128"}