<think>
Okay, so I need to compute the definite integral of x divided by (e^x minus 1) from 0 to infinity. Hmm, I remember that integrals involving exponential functions in the denominator sometimes relate to the Riemann zeta function or maybe the gamma function. Let me think.

First, the integral is ∫₀^∞ x/(e^x - 1) dx. I recall that there's a standard integral formula for ∫₀^∞ x^{s-1}/(e^x - 1) dx which equals Γ(s)ζ(s), where Γ is the gamma function and ζ is the Riemann zeta function. If that's the case, then for our integral, the exponent of x is 1, so s-1 =1, which means s=2. So substituting s=2, the integral should be Γ(2)ζ(2). 

Now, Γ(2) is straightforward. The gamma function Γ(n) for a positive integer n is (n-1)!. So Γ(2) is 1! which is 1. Then ζ(2) is the sum from n=1 to infinity of 1/n². I remember that ζ(2) is π²/6. So putting it all together, the integral should be Γ(2)ζ(2) = 1 * π²/6 = π²/6. 

Wait, let me verify that formula again. The integral ∫₀^∞ x^{s-1}/(e^x -1) dx = Γ(s)ζ(s). Yes, that's correct. So for s=2, it's indeed Γ(2)ζ(2). So the exact answer is π²/6. 

But maybe I should derive it step by step instead of just recalling the formula. Let's try expanding 1/(e^x -1) as a series. Since e^x = 1 + x + x²/2! + ..., so e^x -1 = x + x²/2! + ... which is x(1 + x/2! + x²/3! + ...). But maybe a better approach is to use the expansion 1/(e^x -1) = e^{-x}/(1 - e^{-x}) = Σ_{n=1}^∞ e^{-nx} for x > 0. That's a geometric series expansion. So substituting that into the integral, we get:

∫₀^∞ x/(e^x -1) dx = ∫₀^∞ x Σ_{n=1}^∞ e^{-nx} dx.

Then, interchange the sum and integral (if allowed). By the dominated convergence theorem, since the terms are positive and the series converges, we can swap them. So:

Σ_{n=1}^∞ ∫₀^∞ x e^{-nx} dx.

Now, compute each integral ∫₀^∞ x e^{-nx} dx. Let me make a substitution. Let t = nx, so x = t/n, dx = dt/n. Then the integral becomes:

∫₀^∞ (t/n) e^{-t} (dt/n) = (1/n²) ∫₀^∞ t e^{-t} dt.

The integral ∫₀^∞ t e^{-t} dt is Γ(2) = 1! = 1. So each term is 1/n². Therefore, the sum becomes Σ_{n=1}^∞ 1/n² = ζ(2) = π²/6. So the integral is π²/6. That matches the earlier result. 

So the exact answer is π²/6. Now, for the approximation. π is approximately 3.1415926536, so π² is about 9.8696044011, divided by 6 gives approximately 1.6449340668. Rounded to 10 decimal places, that's 1.6449340668. Let me check with a calculator. π²/6 ≈ 9.8696044 /6 ≈ 1.644934066... yes, that's correct. 

Therefore, the exact answer is π²/6 and the numerical approximation is approximately 1.6449340668.
</think>

{"answer": "\\frac{\\pi^2}{6}", "numerical_answer": 1.6449340668}