<think>
Okay, let's tackle this integral ∫₀² H₃(√(x(2−x))) dx. Hmm, H₃ is the third Hermite polynomial. First, I need to recall what H₃(y) looks like. The Hermite polynomials are given by Hₙ(y) = (-1)ⁿ e^{y²} (d/dy)ⁿ e^{-y²}. Let me write out H₃ explicitly.

The third Hermite polynomial is H₃(y) = 8y³ - 12y. Let me confirm that. Yeah, H₀(y) is 1, H₁(y) is 2y, H₂(y) is 4y² - 2, H₃(y) is 8y³ - 12y. Right. So substituting √(x(2−x)) into H₃, we have H₃(√(x(2−x))) = 8[√(x(2−x))]³ - 12√(x(2−x)).

So the integral becomes ∫₀² [8(x(2−x))^(3/2) - 12(x(2−x))^(1/2)] dx. Let's factor out the constants: 8∫₀² x^(3/2)(2−x)^(3/2) dx - 12∫₀² x^(1/2)(2−x)^(1/2) dx.

Now, these integrals look like Beta functions. The integral ∫₀^a x^{c-1}(a−x)^{d-1} dx = a^{c+d-1} B(c, d), where B is the Beta function. Wait, more precisely, the Beta function is B(p, q) = 2∫₀^(π/2) (sinθ)^{2p-1}(cosθ)^{2q-1} dθ, but also relates to the Gamma function as B(p, q) = Γ(p)Γ(q)/Γ(p+q).

Alternatively, the integral ∫₀^a x^{n}(a−x)^{m} dx = a^{n+m+1} B(n+1, m+1) = a^{n+m+1} Γ(n+1)Γ(m+1)/Γ(n+m+2). Let me check that substitution. Let’s set t = x/a, so x = a t, dx = a dt. Then the integral becomes ∫₀¹ (a t)^n (a(1−t))^m a dt = a^{n+m+1} ∫₀¹ t^n (1−t)^m dt = a^{n+m+1} B(n+1, m+1). Yes, that's correct.

In our case, a = 2. For the first integral, 8∫₀² x^(3/2)(2−x)^(3/2) dx. Here, n = 3/2, m = 3/2. So this becomes 8 * 2^{3/2 + 3/2 +1} B(3/2 +1, 3/2 +1) = 8 * 2^{4} B(5/2, 5/2). Wait, wait, n + m +1 = 3/2 + 3/2 +1 = 4? Wait, no. Wait, the integral is a^{n + m +1} B(n+1, m+1). Wait, in the general formula, the integral is a^{n + m +1} B(n+1, m+1). So here, n and m are the exponents on x and (a−x). So in the first integral, the exponents are 3/2 and 3/2, so n = 3/2, m = 3/2. Then a = 2. So the integral is 2^{3/2 + 3/2 +1} B(3/2 +1, 3/2 +1) = 2^{4} B(5/2, 5/2). Then multiply by 8. So 8 * 2^4 * B(5/2,5/2). Similarly, the second integral is -12 * 2^{1/2 +1/2 +1} B(1/2 +1,1/2 +1) = -12 * 2^{3} B(3/2,3/2).

So let's compute these Beta functions. B(5/2,5/2) = Γ(5/2)Γ(5/2)/Γ(5). Similarly, B(3/2,3/2) = Γ(3/2)^2 / Γ(3).

We know that Γ(1/2) = √π, Γ(3/2) = (1/2)Γ(1/2) = √π/2, Γ(5/2) = (3/2)Γ(3/2) = (3/2)(√π/2) = 3√π/4. Γ(3) = 2! = 2, Γ(5) = 4! = 24.

So B(5/2,5/2) = (3√π/4)^2 / 24? Wait, Γ(5) is 4! = 24. So B(5/2,5/2) = (3√π/4)^2 / 24. Let's compute that: (9π/16) / 24 = 9π/(16*24) = 9π/384 = 3π/128.

Similarly, B(3/2,3/2) = (√π/2)^2 / Γ(3) = (π/4)/2 = π/8.

So now, first integral: 8 * 2^4 * 3π/128. 2^4 is 16. So 8*16 = 128. 128 * 3π/128 = 3π.

Second integral: -12 * 2^3 * π/8. 2^3 is 8. So -12 *8 * π/8 = -12π.

So total integral is 3π -12π = -9π. Wait, that's interesting. So the exact answer is -9π. Let me check the steps again to make sure.

Wait, first integral: 8 * [2^{3/2 +3/2 +1} B(5/2,5/2)]. Wait, 3/2 +3/2 +1 = 3 +1 =4. So 2^4 =16. Then 8*16 =128. Then B(5/2,5/2) is (3√π/4)^2 / Γ(5). Γ(5) is 24. So (9π/16) /24 = 9π/(16*24) = 9π/384 = 3π/128. Then 128 * 3π/128 =3π. Correct.

Second integral: -12 * [2^{1/2 +1/2 +1} B(3/2,3/2)]. 1/2 +1/2 +1 =2. 2^2=4. Then B(3/2,3/2) = (√π/2)^2 / Γ(3) = (π/4)/2 = π/8. So -12 *4 * π/8 = -12*(4/8)*π = -12*(0.5)*π = -6π. Wait, wait, wait. Wait, 2^{1/2 +1/2 +1} is 2^(1 +1) =2^2=4. Then B(3/2,3/2) is π/8. So -12 *4 * π/8 = -12*(4/8)π = -12*(0.5)π = -6π. Wait, but earlier I thought it was -12π. That's a mistake. So the first integral is 3π, the second integral is -6π. So total integral is 3π -6π = -3π. Wait, so I must have made a mistake in the previous calculation. Let me check again.

Wait, the second integral: -12 * ∫₀² x^{1/2}(2−x)^{1/2} dx. So according to the formula, that's 2^{1/2 +1/2 +1} B(1/2 +1,1/2 +1). So exponents are 1/2 and 1/2. So n =1/2, m=1/2. Then a=2. So the integral is 2^{1/2 +1/2 +1} B(3/2,3/2). 1/2 +1/2 +1 =2, so 2^2=4. Then B(3/2,3/2)= Γ(3/2)^2 / Γ(3). Γ(3/2)=√π/2, so squared is π/4. Γ(3)=2. So B(3/2,3/2)= (π/4)/2= π/8. So the integral is 4 * π/8= π/2. Then multiplied by -12: -12*(π/2)= -6π. So first integral is 3π, second is -6π. Total is 3π -6π= -3π. Wait, but earlier I thought the first integral was 3π and the second was -12π. So where did I go wrong?

Ah, in the first calculation, I think I messed up the exponents. Let me recheck:

First integral: 8∫ x^{3/2}(2−x)^{3/2} dx from 0 to 2. So n=3/2, m=3/2. Then the integral is 2^{n + m +1} B(n+1, m+1). Wait, no, the formula is ∫₀^a x^{n} (a−x)^{m} dx = a^{n + m +1} B(n+1, m+1). So here, a=2, n=3/2, m=3/2. So a^{n + m +1} =2^{3/2 +3/2 +1}=2^{4}=16. Then B(n+1, m+1)=B(5/2,5/2)=3π/128 as before. So 16 *3π/128= (16/128)*3π= (1/8)*3π=3π/8. Then multiply by 8: 8*(3π/8)=3π. Correct.

Second integral: -12∫x^{1/2}(2−x)^{1/2}dx. Here, n=1/2, m=1/2. So a^{n +m +1}=2^{1/2 +1/2 +1}=2^2=4. B(n+1, m+1)=B(3/2,3/2)=π/8. So integral is 4*(π/8)=π/2. Multiply by -12: -12*(π/2)= -6π. So total integral is 3π -6π= -3π. So the exact answer is -3π. Wait, but earlier I thought it was -9π. So I must have made a mistake in the first calculation. So the correct answer is -3π. Let me check again.

Wait, so the original integrand is H₃(√(x(2−x))). H₃(y)=8y³−12y. So substituting y=√(x(2−x)), we get 8y³−12y. Then the integral becomes ∫₀² [8y³ -12y] dx, where y=√(x(2−x)}. So 8∫y³ dx -12∫y dx. Then y=√(x(2−x)}= (x(2−x))^{1/2}. So y³=(x(2−x))^{3/2}. So the integrals are ∫x^{3/2}(2−x)^{3/2}dx and ∫x^{1/2}(2−x)^{1/2}dx. So the first integral is 8 times the first Beta function term, and the second is -12 times the second Beta function term.

So the first integral: 8 * [2^{3/2 +3/2 +1} B(5/2,5/2)] =8*16*(3π/128)=3π. The second integral: -12*[2^{1/2 +1/2 +1} B(3/2,3/2)]= -12*4*(π/8)= -6π. So total is 3π -6π= -3π. So exact answer is -3π. Then numerical approximation is -3*3.1415926535...≈-9.42477796077. Rounded to 10 decimal places, that's -9.4247779608.

Wait, but let me confirm the Beta function calculations again. For B(5/2,5/2)=Γ(5/2)^2 / Γ(5). Γ(5/2)= (3/2)(1/2)√π= (3/4)√π. So Γ(5/2)^2= (9/16)π. Γ(5)=24. So B(5/2,5/2)= (9/16 π)/24=9π/(16*24)=9π/384=3π/128. Yes. Then 8*3π/128*16? Wait, no. Wait, the integral is 8* [2^{4} * B(5/2,5/2)] =8*16*(3π/128)=8*16*3π/(128). 16/128=1/8. So 8*(1/8)*3π=3π. Correct.

Similarly, B(3/2,3/2)=Γ(3/2)^2 / Γ(3). Γ(3/2)= (1/2)√π. So squared is π/4. Γ(3)=2. So B(3/2,3/2)= (π/4)/2=π/8. Then the integral is -12*[2^{2} * π/8]=-12*(4*π/8)= -12*(π/2)= -6π. Correct. So the exact answer is -3π. Therefore, the numerical approximation is -3*π≈-9.42477796077, which rounds to -9.4247779608.

But wait, let me compute π to more decimal places. π≈3.141592653589793. So -3π≈-9.42477796076938. Rounded to 10 decimal places, that's -9.4247779608.

So the final answer is {"answer": "-3\\pi", "numerical_answer": "-9.4247779608"}.
</think>

{"answer": "-3\\pi", "numerical_answer": "-9.4247779608"}