<think>
Okay, let's see. I need to compute the definite integral of 1/(3^x + 1) from -1 to 1. Hmm, I remember that sometimes with integrals involving exponentials in the denominator, substitution might help. Let me think.

First, maybe I can simplify the integrand. The function is 1/(3^x + 1). Let me consider substitution. Let’s set u = -x. Then, when x = -1, u = 1, and when x = 1, u = -1. The differential du would be -dx, so dx = -du. Let's try substituting:

Integral from x=-1 to x=1 of 1/(3^x + 1) dx becomes integral from u=1 to u=-1 of 1/(3^{-u} + 1) (-du). Flipping the limits, that's integral from u=-1 to u=1 of 1/(3^{-u} + 1) du. But 3^{-u} is the same as (1/3)^u. So the integrand is 1/( (1/3)^u + 1 ). Let me write that as 1/(1 + (1/3)^u ). Hmm, maybe I can express this in terms of 3^u. Let's see: (1/3)^u = 3^{-u}, so 1 + 3^{-u} = 3^{-u} + 1. Wait, that's the same as the original integrand but with u instead of x. Wait, but this seems like it's leading me to the same expression. Maybe there's a symmetry here.

Wait, let me write the original integral as I(-1,1) 1/(3^x +1) dx and the transformed integral after substitution as I(-1,1) 1/(3^{-u} +1) du. Let me add these two expressions. If I call the original integral I, then after substitution, the transformed integral is also I. So I + I would be the integral from -1 to 1 of [1/(3^x +1) + 1/(3^{-x} +1)] dx. Let me compute that sum inside the integral.

1/(3^x +1) + 1/(3^{-x} +1) = [1/(3^x +1)] + [1/(1/(3^x) +1)]. Let me compute the second term: 1/(1/(3^x) +1) = 1/( (1 + 3^x)/3^x ) = 3^x/(1 + 3^x). So adding the two terms: [1/(3^x +1)] + [3^x/(3^x +1)] = (1 + 3^x)/(3^x +1) = 1. So the sum is 1. Therefore, I + I = integral from -1 to 1 of 1 dx = 2. So 2I = 2, which implies I = 1. Wait, that can't be right. Wait, the integral from -1 to 1 of 1 dx is 2, so 2I = 2, so I = 1. Hmm, that seems too simple. Let me check.

Wait, let me verify this. If I have the original integral I = ∫_{-1}^1 1/(3^x +1) dx. Then, after substitution u = -x, we get I = ∫_{-1}^1 1/(3^{-u} +1) du. Then adding the two expressions: I + I = ∫_{-1}^1 [1/(3^x +1) + 1/(3^{-x} +1)] dx. Then, as shown earlier, the integrand simplifies to 1. Therefore, the integral becomes ∫_{-1}^1 1 dx = 2. So 2I = 2 => I = 1. So the exact answer is 1? That seems surprising. Let me check with a numerical approximation.

Alternatively, maybe I made a mistake in the substitution step. Let me try another approach. Let's compute the integral directly. Let’s consider the integral ∫1/(3^x +1) dx. Let me make a substitution. Let’s set t = 3^x. Then, ln t = x ln 3, so dx = dt/(t ln 3). Then, the integral becomes ∫1/(t +1) * (dt)/(t ln 3) = (1/ln 3) ∫ dt/(t(t +1)). That can be split into partial fractions. Let's write 1/(t(t +1)) as A/t + B/(t +1). Solving, 1 = A(t +1) + Bt. Let t = -1: 1 = A(0) + B(-1) => B = -1. Let t = 0: 1 = A(1) + B(0) => A = 1. So, 1/(t(t +1)) = 1/t - 1/(t +1). Therefore, the integral becomes (1/ln 3) [ ∫1/t dt - ∫1/(t +1) dt ] = (1/ln 3) [ ln |t| - ln |t +1| ] + C. Substitute back t = 3^x: (1/ln 3) [ ln(3^x) - ln(3^x +1) ] + C. Simplify ln(3^x) = x ln 3. So, the integral is (1/ln 3)[x ln 3 - ln(3^x +1)] + C = x - (1/ln 3) ln(3^x +1) + C.

Now, evaluate from -1 to 1. So, the definite integral is [1 - (1/ln 3) ln(3^1 +1)] - [ -1 - (1/ln 3) ln(3^{-1} +1) ].

Simplify each term:

First term at upper limit 1: 1 - (1/ln 3) ln(4).

Second term at lower limit -1: -1 - (1/ln 3) ln(1/3^{-1} +1). Wait, 3^{-1} is 1/3, so 1/3 +1 = 4/3. So ln(4/3). So the lower limit term is -1 - (1/ln 3) ln(4/3).

Putting it all together:

[1 - (1/ln 3) ln(4)] - [ -1 - (1/ln 3) ln(4/3) ] = 1 - (ln4)/ln3 +1 + (ln(4/3))/ln3.

Combine terms: 2 + [ (ln(4/3) - ln4) ] / ln3.

Simplify the logarithm terms: ln(4/3) - ln4 = ln( (4/3)/4 ) = ln(1/3) = -ln3.

Therefore, the expression becomes 2 + (-ln3)/ln3 = 2 -1 = 1. So the integral is 1. So that matches the previous result. Therefore, the exact answer is 1.

Wait, that's interesting. So the integral from -1 to 1 of 1/(3^x +1) dx equals 1. Let me check with approximate numerical value. Let's compute the integral numerically. Let's compute the integral from -1 to 1 of 1/(3^x +1) dx. Let's split it into two parts: from -1 to 0 and 0 to 1.

First, from -1 to 0: 3^x is 3^(-1) to 3^0, which is 1/3 to 1. The integrand 1/(3^x +1) at x=-1: 1/(1/3 +1) = 3/4. At x=0: 1/(1 +1) = 1/2. The function is decreasing here. The integral over this interval can be approximated as the average of the endpoints times the interval length (0 - (-1))=1. But that's trapezoidal rule with two points. The approximate value would be (3/4 +1/2)/2 *1 = (5/4)/2 = 5/8 = 0.625.

Similarly, from 0 to1: 3^x goes from 1 to 3. The integrand at x=0 is 1/2, at x=1 is 1/(3 +1)=1/4. Again, decreasing. The average would be (1/2 +1/4)/2 *1 = (3/4)/2 = 3/8=0.375. So total approximate integral is 0.625 +0.375=1. So that matches the exact result. So the numerical approximation is 1.0000000000. But wait, maybe the exact answer is 1. Let me check with another method.

Alternatively, use substitution. Let’s see, when I did the substitution u = -x, and added the two integrals, I got 2I = 2, so I=1. So the exact answer is 1, and the approximation is exactly 1.0000000000. But wait, maybe the exact answer is exactly 1. Let me confirm with another example. Suppose I take the integral from -a to a of 1/(k^x +1) dx. Using the same method, substitution u = -x, then adding the two integrals, the sum would be integral from -a to a of 1 dx = 2a. So 2I = 2a => I =a. Wait, but that would mean that for any a, the integral from -a to a of 1/(k^x +1) dx =a. That seems too general. Wait, but in our case, a=1, k=3, so the integral is 1. But let me check with k=2, a=1. Let's compute ∫_{-1}^1 1/(2^x +1) dx. Using the same method: substitution u=-x, then adding the integrals, we get 2I = ∫_{-1}^1 1 dx =2, so I=1. But let's compute it directly. Let's compute the integral from -1 to1 of 1/(2^x +1) dx. Let's compute numerically. From x=-1 to 0: 2^x from 0.5 to1. The integrand at x=-1:1/(0.5 +1)=2/3≈0.6667, at x=0:1/2=0.5. The approximate integral using trapezoidal: (0.6667 +0.5)/2 *1 ≈0.5833. From 0 to1: 2^x from1 to2. Integrand at x=0:0.5, at x=1:1/3≈0.3333. Trapezoidal: (0.5 +0.3333)/2 *1≈0.4166. Total≈0.5833+0.4166≈1. So again, the integral is 1. So this seems to be a general result: ∫_{-a}^a 1/(k^x +1) dx =a. Wait, that's fascinating. So for any a and any positive k≠1, the integral from -a to a of 1/(k^x +1) dx equals a. That's a neat symmetry. So in our case, a=1, so the integral is 1. Therefore, the exact answer is 1, and the numerical approximation is exactly 1.0000000000. So the problem is designed to have this symmetry leading to an exact integer result. Therefore, the answer is 1.
</think>

{"answer": "1", "numerical_answer": "1.0000000000"}