We start with the given integral

  I = ∫ from e to e^e ( (log x)·(log(log x)) / x ) dx.

Step 1. Substitute u = log x.
  Then, du = (1/x) dx  ⟹  dx = x du = e^u du.
  When x = e, u = log e = 1; and when x = e^e, u = log(e^e) = e.
  The integrand becomes:
   (log x) = u and (log(log x)) = log u and (1/x dx) = du.
Thus, the integral simplifies to:
  I = ∫ from u = 1 to u = e ( u·log u ) du.

Step 2. Evaluate I = ∫ u log u du.
Use integration by parts:
  Let v = log u ⟹ dv = (1/u) du,
  and let dw = u du ⟹ w = u²/2.
Then,
  ∫ u log u du = w·v − ∫ w dv
            = (u²/2) log u − ∫ (u²/2)(1/u) du
            = (u²/2) log u − (1/2) ∫ u du
            = (u²/2) log u − (1/2)(u²/2) + C
            = (u²/2) log u − u²/4 + C.

Now, evaluate from u = 1 to u = e:
 At u = e: (e²/2) log(e) − e²/4 = (e²/2)(1) − e²/4 = e²/2 − e²/4 = e²/4.
 At u = 1: (1²/2) log(1) − 1²/4 = 0 − 1/4 = −1/4.
Thus,
 I = [e²/4 − (−1/4)] = (e²/4 + 1/4) = (e² + 1)/4.

Step 3. Numerical Approximation.
Calculate:
 e² ≈ 7.389056099,
 Then, (e² + 1)/4 ≈ (7.389056099 + 1) / 4 ≈ 8.389056099 / 4 ≈ 2.0972640248.

Final Answer in JSON format:
{"answer": "\\frac{e^2+1}{4}", "numerical_answer": "2.0972640248"}