We wish to evaluate

  I = ∫₋₄⁴ e^(|x|) {x} dx,

where {x} is the fractional part of x. (Recall that for any real number x, if n = ⎣x⎦ then {x} = x – n and always 0 ≤ {x} < 1.)

Step 1. Split the interval into unit‐intervals.
Because the fractional part is defined in a piecewise‐fashion, we break [–4, 4] into the eight subintervals
  [–4, –3), [–3, –2), [–2, –1), [–1, 0), [0, 1), [1, 2), [2, 3), [3, 4].
In a generic interval [n, n+1) (with integer n) we have
  {x} = x – n.
Observe that for x < 0 (i.e. when n is negative) we have |x| = –x, while for x ≥ 0 we have |x| = x.

Thus, we write the integral as the sum over individual intervals:
  I = Σₙ₌₋₄⁻¹ ∫ₙⁿ⁺¹ e^(–x) (x – n) dx + Σₙ₌₀³ ∫ₙⁿ⁺¹ e^x (x – n) dx.

Step 2. Change of variable on each interval.
For each interval let u = x – n. Then x = n + u and du = dx. Notice that when x runs from n to n + 1, u goes from 0 to 1. Thus, the integrals become:

For n negative:
  Iₙ = ∫₀¹ e^(–(n+u)) u du = e^(–n) ∫₀¹ u e^(–u) du.
For n nonnegative:
  Iₙ = ∫₀¹ e^(n+u) u du = e^n ∫₀¹ u e^u du.

We now define
  A = ∫₀¹ u e^(–u) du  and  B = ∫₀¹ u e^u du.

Step 3. Compute A and B.
To compute A, integrate by parts or use a known antiderivative. One can show that
  ∫ u e^(–u) du = –e^(–u)(u + 1) + C.
Thus,
  A = [–e^(–u)(u + 1)]₀¹ = [ –e^(–1)(1 + 1) ] – [ –e^(0)(0 + 1) ]
       = –2e^(–1) + 1 = 1 – 2/e.

Similarly, for B we have
  ∫ u e^u du = e^u(u – 1) + C,
so that
  B = [e^u(u – 1)]₀¹ = [e^(1)(1 – 1)] – [e^(0)(0 – 1)] = 0 – (–1) = 1.

Step 4. Rewrite the full sum.
The contributions become

• For the negative intervals (n = –4, –3, –2, –1):
  Σₙ₌₋₄⁻¹ e^(–n) A = A [e^(–(–4)) + e^(–(–3)) + e^(–(–2)) + e^(–(–1))]
       = A (e⁴ + e³ + e² + e).

• For the nonnegative intervals (n = 0, 1, 2, 3):
  Σₙ₌₀³ e^n B = (1 + e + e² + e³).

Thus,
  I = A (e + e² + e³ + e⁴) + (1 + e + e² + e³).

Substitute A = 1 – 2/e:
  I = (1 – 2/e)(e + e² + e³ + e⁴) + (1 + e + e² + e³).

Step 5. Simplify the expression.
Let S = e + e² + e³ + e⁴ and let T = 1 + e + e² + e³. Notice that S = e(1 + e + e² + e³) = eT. Then
  I = S – (2/e) S + T = eT – (2T) + T = T(e – 2 + 1) = T (e – 1).

Since T = 1 + e + e² + e³ and this is a geometric series with ratio e, we have
  1 + e + e² + e³ = (e⁴ – 1)/(e – 1).
Then
  I = ( (e⁴ – 1)/(e – 1) ) (e – 1) = e⁴ – 1.

Step 6. Provide the numerical approximation.
We have
  I = e⁴ – 1.
Using e ≈ 2.7182818285, we compute
  e⁴ ≈ 54.5981500331,
so the numerical value is
  I ≈ 54.5981500331 – 1 = 53.5981500331.
Rounded to 10 decimal places, I ≈ 53.5981500331.

Finally, we output the result in the required JSON format.

{"answer": "$e^4 - 1$", "numerical_answer": "53.5981500331"}