

To solve the definite integral \(\int_0^1 \sin^2(\log x) \, dx\), we proceed as follows:

### Step 1: Substitution
Let \( t = \log x \). Then \( x = e^t \) and \( dx = e^t \, dt \). When \( x = 0 \), \( t \to -\infty \); when \( x = 1 \), \( t = 0 \). The integral transforms to:
\[
\int_{-\infty}^0 \sin^2(t) \cdot e^t \, dt
\]

### Step 2: Use Trigonometric Identity
Recall the identity \( \sin^2(t) = \frac{1 - \cos(2t)}{2} \). Substituting this into the integral gives:
\[
\int_{-\infty}^0 \frac{1 - \cos(2t)}{2} \cdot e^t \, dt = \frac{1}{2} \int_{-\infty}^0 e^t \, dt - \frac{1}{2} \int_{-\infty}^0 \cos(2t) \cdot e^t \, dt
\]

### Step 3: Evaluate the First Integral
The first integral is straightforward:
\[
\int_{-\infty}^0 e^t \, dt = \left. e^t \right|_{-\infty}^0 = e^0 - \lim_{t \to -\infty} e^t = 1 - 0 = 1
\]

### Step 4: Evaluate the Second Integral
For the second integral, we use integration by parts or recognize it as a Laplace transform. Let \( I = \int_{-\infty}^0 \cos(2t) \cdot e^t \, dt \). Substitute \( u = -t \) (so \( t = -u \), \( dt = -du \)), transforming the limits to \( u \to \infty \) (when \( t \to -\infty \)) and \( u = 0 \) (when \( t = 0 \)):
\[
I = \int_{\infty}^0 \cos(-2u) \cdot e^{-u} (-du) = \int_0^\infty \cos(2u) \cdot e^{-u} \, du
\]
This is the Laplace transform of \( \cos(2u) \) evaluated at \( s = 1 \). The Laplace transform of \( \cos(at) \) is \( \frac{s}{s^2 + a^2} \), so:
\[
I = \left. \frac{s}{s^2 + (2)^2} \right|_{s=1} = \frac{1}{1^2 + 2^2} = \frac{1}{5}
\]

### Step 5: Combine Results
Substituting back, the original integral becomes:
\[
\frac{1}{2} \left( 1 - \frac{1}{5} \right) = \frac{1}{2} \cdot \frac{4}{5} = \frac{2}{5}
\]

### Numerical Approximation
The exact value is \( \frac{2}{5} \), which is \( 0.4 \) when rounded to 10 decimal places.

{"answer": "\\frac{2}{5}", "numerical_answer": "0.4000000000"}