We wish to evaluate

  I = ∫₍π/6₎^(π/3) (sin x + cos x)⁄√(sin 2x) dx.

Step 1. Rewrite the integrand.

Notice that sin 2x = 2 sin x cos x so that
  √(sin 2x) = √(2 sin x cos x) = √2 · √(sin x cos x)      (when sin x and cos x are positive, as they are on [π/6, π/3]).

A key observation is that
  d/dx [sin x – cos x] = cos x + sin x.
That is, the numerator is exactly the derivative of (sin x – cos x).

Step 2. Use a substitution.

Let
  u = sin x – cos x.
Then,
  du = (sin x + cos x) dx.
Thus the given integral becomes
  I = ∫ (du)⁄√(sin 2x).

Now we must express √(sin 2x) in terms of u.

Note that
  u² = (sin x – cos x)² = sin²x – 2 sin x cos x + cos²x = 1 – 2 sin x cos x.
That is,
  2 sin x cos x = 1 – u².
Since sin 2x = 2 sin x cos x we have
  √(sin 2x) = √(1 – u²).

Thus the integral becomes
  I = ∫ du/√(1 – u²),
with the new limits computed from:
  When x = π/6: u = sin(π/6) – cos(π/6) = ½ – (√3⁄2) = (1 – √3)/2.
  When x = π/3: u = sin(π/3) – cos(π/3) = (√3⁄2) – ½ = (√3 – 1)/2.

Step 3. Evaluate the new integral.

We recognize that
  ∫ du/√(1 – u²) = arcsin u + C.
So,
  I = arcsin u |₍u=(1–√3)/2₎^(u=(√3–1)/2)
    = arcsin((√3 – 1)/2) – arcsin((1 – √3)/2).

But note that arcsin is an odd function, i.e. arcsin(–a) = –arcsin(a). Since
  (1 – √3)/2 = –((√3 – 1)/2),
we have
  arcsin((1 – √3)/2) = – arcsin((√3 – 1)/2).
Thus,
  I = arcsin((√3 – 1)/2) – [– arcsin((√3 – 1)/2)]
    = 2 · arcsin((√3 – 1)/2).

This is the exact answer.

Step 4. Numerical approximation.

We now compute the numerical value. Define
  z = (√3 – 1)/2.
Since √3 ≈ 1.7320508075688772, then
  z ≈ (1.7320508075688772 – 1)/2 ≈ 0.3660254037844386.

We need to compute A = arcsin(z). Using a power series (or a calculator) we find
  arcsin(0.3660254037844386) ≈ 0.37472387  (in radians).
Thus,
  I = 2A ≈ 2 × 0.37472387 ≈ 0.74944774.

Step 5. Final Answer in JSON Format

{"answer": "2\\arcsin\\left(\\frac{\\sqrt{3}-1}{2}\\right)", "numerical_answer": "0.7494477400"}