To solve the definite integral 

\[
\int_0^{\frac{\pi}{4}} \tan^{-1}\left(\frac{1 + \tan(x)}{\sqrt{2}}\right) \mathrm{d}x,
\]

we will follow these steps:

### Step 1: Simplify the Integrand
First, let's simplify the argument of the arctangent function. Notice that:

\[
\frac{1 + \tan(x)}{\sqrt{2}} = \frac{\sin(x) + \cos(x)}{\sqrt{2} \cdot \frac{1}{\cos(x)} = \frac{\sin\left(x + \frac{\pi}{4}\right)}{\cos(x)},
\]

where we used the identity \(\sin(x) + \cos(x) = \sqrt{2} \sin\left(x + \frac{\pi}{4}\right)\). However, this simplification might not directly help, so we consider an alternative approach.

### Step 2: Substitution
Let’s make the substitution:

\[
u = \tan(x) \quad \Rightarrow \quad \mathrm{d}u = \sec^2(x) \mathrm{d}x = (1 + \tan^2(x)) \mathrm{d}x.
\]

When \(x = 0\), \(u = 0\), and when \(x = \frac{\pi}{4}\), \(u = 1\). The integral becomes:

\[
\int_0^1 \tan^{-1}\left(\frac{1 + u}{\sqrt{2}}\right) \cdot \frac{\mathrm{d}u}{1 + u^2}.
\]

### Step 3: Integration by Parts
Let’s set:

\[
I = \int_0^1 \tan^{-1}\left(\frac{1 + u}{\sqrt{2}}\right) \cdot \frac{\mathrm{d}u}{1 + u^2}.
\]

We can use integration by parts with:

\[
v = \tan^{-1}\left(\frac{1 + u}{\sqrt{2}}\right), \quad \mathrm{d}w = \frac{\mathrm{d}u}{1 + u^2}.
\]

Then:

\[
\mathrm{d}v = \frac{1}{1 + \left(\frac{1 + u}{\sqrt{2}}\right)^2} \cdot \frac{1}{\sqrt{2}} \mathrm{d}u = \frac{\sqrt{2}}{2 + (1 + u)^2} \mathrm{d}u,
\]

and \(w = \tan^{-1}(u)\). Applying integration by parts:

\[
I = \left. \tan^{-1}(u) \tan^{-1}\left(\frac{1 + u}{\sqrt{2}}\right) \right|_0^1 - \int_0^1 \tan^{-1}(u) \cdot \frac{\sqrt{2}}{2 + (1 + u)^2} \mathrm{d}u.
\]

Evaluating the boundary term:

\[
\left. \tan^{-1}(u) \tan^{-1}\left(\frac{1 + u}{\sqrt{2}}\right) \right|_0^1 = \frac{\pi}{4} \cdot \tan^{-1}\left(\frac{2}{\sqrt{2}}\right) - 0 = \frac{\pi}{4} \cdot \frac{\pi}{4} = \frac{\pi^2}{16},
\]

since \(\tan^{-1}\left(\frac{2}{\sqrt{2}}\right) = \tan^{-1}(\sqrt{2}) = \frac{\pi}{4}\) (this is incorrect; actually, \(\tan^{-1}(\sqrt{2})\) is not \(\frac{\pi}{4}\). Let's correct this.)

Actually, \(\tan^{-1}\left(\frac{2}{\sqrt{2}}\right) = \tan^{-1}(\sqrt{2})\), which is not a standard angle. This suggests that integration by parts may not be the best approach here.

### Step 4: Alternative Approach - Differentiating Under the Integral
Consider the integral as a function of a parameter. Let:

\[
I(a) = \int_0^{\frac{\pi}{4}} \tan^{-1}\left(\frac{a + \tan(x)}{\sqrt{2}}\right) \mathrm{d}x.
\]

We want \(I(1)\). Differentiate \(I(a)\) with respect to \(a\):

\[
I'(a) = \int_0^{\frac{\pi}{4}} \frac{1}{1 + \left(\frac{a + \tan(x)}{\sqrt{2}}\right)^2} \cdot \frac{1}{\sqrt{2}} \mathrm{d}x = \int_0^{\frac{\pi}{4}} \frac{\sqrt{2}}{2 + (a + \tan(x))^2} \mathrm{d}x.
\]

This seems complicated, so let's try another substitution.

### Step 5: Substitution \(x = \frac{\pi}{4} - t\)
Let \(x = \frac{\pi}{4} - t\), then \(\mathrm{d}x = -\mathrm{d}t\), and the integral becomes:

\[
I = \int_{\frac{\pi}{4}}^0 \tan^{-1}\left(\frac{1 + \tan\left(\frac{\pi}{4} - t\right)}{\sqrt{2}}\right) (-\mathrm{d}t) = \int_0^{\frac{\pi}{4}} \tan^{-1}\left(\frac{1 + \frac{1 - \tan(t)}{1 + \tan(t)}}{\sqrt{2}}\right) \mathrm{d}t.
\]

Simplify the argument:

\[
\frac{1 + \frac{1 - \tan(t)}{1 + \tan(t)}}{\sqrt{2}} = \frac{\frac{(1 + \tan(t)) + (1 - \tan(t))}{1 + \tan(t)}}{\sqrt{2}} = \frac{\frac{2}{1 + \tan(t)}}{\sqrt{2}} = \frac{\sqrt{2}}{1 + \tan(t)}.
\]

Thus, the integral becomes:

\[
I = \int_0^{\frac{\pi}{4}} \tan^{-1}\left(\frac{\sqrt{2}}{1 + \tan(t)}\right) \mathrm{d}t.
\]

Now, add the original integral \(I\) and this transformed integral:

\[
2I = \int_0^{\frac{\pi}{4}} \left[ \tan^{-1}\left(\frac{1 + \tan(t)}{\sqrt{2}}\right) + \tan^{-1}\left(\frac{\sqrt{2}}{1 + \tan(t)}\right) \right] \mathrm{d}t.
\]

Using the identity \(\tan^{-1}(a) + \tan^{-1}\left(\frac{1}{a}\right) = \frac{\pi}{2}\) for \(a > 0\), we have:

\[
\tan^{-1}\left(\frac{1 + \tan(t)}{\sqrt{2}}\right) + \tan^{-1}\left(\frac{\sqrt{2}}{1 + \tan(t)}\right) = \frac{\pi}{2}.
\]

Therefore:

\[
2I = \int_0^{\frac{\pi}{4}} \frac{\pi}{2} \mathrm{d}t = \frac{\pi}{2} \cdot \frac{\pi}{4} = \frac{\pi^2}{8},
\]

so:

\[
I = \frac{\pi^2}{16}.
\]

### Numerical Approximation
The numerical value of \(\frac{\pi^2}{16}\) is approximately:

\[
\frac{\pi^2}{16} \approx 0.6168502751.
\]

### Final Answer
```json
{"answer": "\\frac{\\pi^2}{16}", "numerical_answer": "0.6168502751"}
```