
To solve the definite integral \(\int_{0}^{1} x^{-3/4}(1-x)^{-1/4}\left[1 - \sqrt{x(1-x)}\right]^{-2} \, dx\), we proceed with the following steps:


### Step 1: Substitution to Simplify the Integrand
We start by using the substitution \( t = \sqrt{\frac{x}{1-x}} \), which implies \( x = \frac{t^2}{1+t^2} \) and \( dx = \frac{2t}{(1+t^2)^2} \, dt \). This transforms the original integral into a more manageable form. 

Under this substitution:
- \( x^{-3/4} = \left(\frac{t^2}{1+t^2}\right)^{-3/4} = \frac{(1+t^2)^{3/4}}{t^{3/2}} \)
- \( (1-x)^{-1/4} = \left(\frac{1}{1+t^2}\right)^{-1/4} = (1+t^2)^{1/4} \)
- \( \sqrt{x(1-x)} = \frac{t}{1+t^2} \)

Substituting these into the integrand and simplifying, the integral becomes:
\[
\int_{0}^{\infty} \frac{2(1+t^2)}{\sqrt{t}(t^2 - t + 1)^2} \, dt
\]


### Step 2: Further Substitution and Simplification
Next, we use \( t = s^2 \) (so \( dt = 2s \, ds \) and \( \sqrt{t} = s \)), which transforms the integral into:
\[
4 \int_{0}^{\infty} \frac{1+s^4}{(s^4 - s^2 + 1)^2} \, ds
\]


### Step 3: Splitting the Integrand
We split the integrand using \( 1+s^4 = (s^4 - s^2 + 1) + s^2 \), leading to:
\[
4 \left( \int_{0}^{\infty} \frac{1}{s^4 - s^2 + 1} \, ds + \int_{0}^{\infty} \frac{s^2}{(s^4 - s^2 + 1)^2} \, ds \right)
\]


### Step 4: Evaluating the Integrals
- For the first integral \( I = \int_{0}^{\infty} \frac{1}{s^4 - s^2 + 1} \, ds \), we use symmetry and substitution to find \( I = \frac{\pi}{2} \).
- For the second integral \( J = \int_{0}^{\infty} \frac{s^2}{(s^4 - s^2 + 1)^2} \, ds \), we use differentiation under the integral sign (parameter differentiation) to find \( J = \frac{\pi}{4} \).


### Step 5: Combining Results
Adding these results and multiplying by 4, we get:
\[
4 \left( \frac{\pi}{2} + \frac{\pi}{4} \right) = 3\pi
\]


### Numerical Approximation
The numerical value of \( 3\pi \) is approximately \( 9.4247779608 \).


{"answer": "3\\pi", "numerical_answer": "9.4247779608"}