Let's carefully solve the integral:
\[
I = \int_0^1 \left( \frac{1}{x} - \left\lfloor \frac{1}{x} \right\rfloor \right) dx.
\]

**Step 1: Split the integral into intervals.**

For \(x \in (0,1]\), \(\frac{1}{x}\) is in \([1, \infty)\).
For \(n \in \mathbb{N}\), for \(x \in \left(\frac{1}{n+1}, \frac{1}{n}\right]\), we have \(n < \frac{1}{x} \leq n+1\). So, \(\left\lfloor \frac{1}{x} \right\rfloor = n\) for \(x \in \left(\frac{1}{n+1}, \frac{1}{n}\right]\).

So,
\[
I = \sum_{n=1}^{\infty} \int_{\frac{1}{n+1}}^{\frac{1}{n}} \left( \frac{1}{x} - n \right) dx.
\]

**Step 2: Compute the integral for a fixed \( n \).**

\[
\int_{\frac{1}{n+1}}^{\frac{1}{n}} \left( \frac{1}{x} - n \right) dx =
\int_{\frac{1}{n+1}}^{\frac{1}{n}} \frac{1}{x} dx - n \int_{\frac{1}{n+1}}^{\frac{1}{n}} dx
\]
\[
= \left. \ln x \right|_{\frac{1}{n+1}}^{\frac{1}{n}} - n \left( \frac{1}{n} - \frac{1}{n+1} \right )
\]
\[
= \left( \ln \frac{1}{n} - \ln \frac{1}{n+1} \right ) - n \left( \frac{1}{n(n+1)} \right)
\]
\[
= \ln \left( \frac{n+1}{n} \right ) - \frac{1}{n+1}
\]

**Step 3: Write the sum.**

\[
I = \sum_{n=1}^{\infty} \left( \ln \frac{n+1}{n} - \frac{1}{n+1} \right )
\]

\[
= \sum_{n=1}^{\infty} \ln \left ( 1 + \frac{1}{n} \right ) - \sum_{n=2}^\infty \frac{1}{n}
\]
(The second sum is shifted in index.)

The first sum:
\[
\sum_{n=1}^{\infty} \ln \left( 1 + \frac{1}{n} \right ) = \sum_{n=1}^\infty \left [ \ln(n+1) - \ln(n) \right ] = \lim_{N \to \infty} (\ln(N+1) - \ln(1)) = \infty
\]
But the difference with the harmonic series will remain finite.

*Actually, letâ€™s sum as below:*
\[
I = \sum_{n=1}^{\infty} \ln\left(1 + \frac{1}{n}\right) - \sum_{n=2}^\infty \frac{1}{n}
= \sum_{n=1}^\infty [\ln(n+1) - \ln(n)] - \sum_{n=2}^\infty \frac{1}{n}
\]
\[
= \lim_{N \to \infty} \left [\ln(N+1) - \ln(1) - \sum_{n=2}^N \frac{1}{n} \right ]
\]
But the harmonic sum diverges as \(\ln N + \gamma\), where \(\gamma\) is Euler-Mascheroni constant:
\[
\sum_{n=1}^N \frac{1}{n} = \ln N + \gamma + \frac{1}{2N} + O(N^{-2}).
\]
So,
\[
\sum_{n=2}^N \frac{1}{n} = \sum_{n=1}^N \frac{1}{n} - 1 = (\ln N + \gamma) - 1
\]
And,
\[
I_N = \ln(N+1) - \sum_{n=2}^N \frac{1}{n}
= \ln(N+1) - (\ln N + \gamma - 1)
= \ln(N+1) - \ln N - \gamma + 1
\]
\[
= \ln \left( 1 + \frac{1}{N} \right ) - \gamma + 1
\]
So
\[
\lim_{N\to\infty} I_N = 0 - \gamma + 1 = 1 - \gamma
\]

**Step 4: Numerical approximation**

\[
\gamma \approx 0.5772156649
\]
So,
\[
I \approx 1 - 0.5772156649 = 0.4227843351
\]

**Step 5: Final answer**

```json
{"answer": "1 - \\gamma", "numerical_answer": "0.4227843351"}
```