# Evaluating $\int\limits_0^1\frac1{1+x^2}\arctan\left(x^{13+\sqrt{168}}\right)dx$

I'll approach this integral by using substitution and properties of definite integrals.

## Step 1: Let's denote $\alpha = 13+\sqrt{168}$ for simplicity.

So we're calculating $\int\limits_0^1\frac1{1+x^2}\arctan\left(x^{\alpha}\right)dx$.

## Step 2: Make the substitution $u = \arctan(x)$

When $u = \arctan(x)$:
- $x = \tan(u)$
- $dx = \sec^2(u) \, du$
- When $x = 0$, $u = 0$
- When $x = 1$, $u = \pi/4$

The integral becomes:
$$\int\limits_0^{\pi/4}\frac{\sec^2(u)}{1+\tan^2(u)}\arctan\left(\tan^{\alpha}(u)\right)du$$

Since $1+\tan^2(u) = \sec^2(u)$, this simplifies to:
$$\int\limits_0^{\pi/4}\arctan\left(\tan^{\alpha}(u)\right)du$$

## Step 3: Use the property of $\tan$ raised to a power

For $0 < u < \pi/4$, we know that $0 < \tan(u) < 1$. When we raise a number between 0 and 1 to a power greater than 1 (which $\alpha$ is), the result gets smaller. Therefore:
$$\tan^{\alpha}(u) < \tan(u)$$

Since $\arctan$ is an increasing function, we have:
$$\arctan(\tan^{\alpha}(u)) = \tan^{\alpha}(u)$$

This is because $\tan^{\alpha}(u)$ is already in the range of $\arctan$ for the values of $u$ we're considering.

## Step 4: Our integral becomes
$$\int\limits_0^{\pi/4}\tan^{\alpha}(u)du$$

## Step 5: Use the key integral formula

It can be proven that:
$$\int_0^{\pi/4} \tan^s(x) dx = \frac{\pi}{4} - \frac{1}{2}\int_0^1 \frac{t^{(s-1)/2}}{1+t} dt$$

where this formula is valid for $s > 0$.

With $s = \alpha = 13+\sqrt{168}$, we get:
$$\int_0^{\pi/4} \tan^{\alpha}(u) du = \frac{\pi}{4} - \frac{1}{2}\int_0^1 \frac{t^{(\alpha-1)/2}}{1+t} dt$$

## Step 6: Evaluate the remaining integral

The integral $\int_0^1 \frac{t^{(\alpha-1)/2}}{1+t} dt$ has a special form. 

Let $\beta = \frac{\alpha-1}{2} = \frac{13+\sqrt{168}-1}{2} = \frac{12+\sqrt{168}}{2} = 6+\frac{\sqrt{168}}{2}$

This integral equals:
$$\int_0^1 \frac{t^{\beta}}{1+t} dt = \sum_{k=0}^{\infty} (-1)^k \frac{1}{\beta+1+k}$$

## Step 7: The final answer

The exact value of our original integral is:
$$\frac{\pi}{4} - \frac{1}{2}\sum_{k=0}^{\infty} \frac{(-1)^k}{\beta+1+k}$$

where $\beta = 6+\frac{\sqrt{168}}{2}$.

This can be expressed in terms of the digamma function $\psi$:
$$\frac{\pi}{4} - \frac{1}{2}\left[\psi\left(\frac{\beta+2}{2}\right) - \psi\left(\frac{\beta+1}{2}\right)\right]$$

With $\beta = 6+\frac{\sqrt{168}}{2}$, and calculating numerically:

$$\frac{\pi}{4} - \frac{1}{2}\left[\psi\left(\frac{7+\frac{\sqrt{168}}{2}}{2}\right) - \psi\left(\frac{6+\frac{\sqrt{168}}{2}+1}{2}\right)\right] = \frac{\pi}{4} - \frac{1}{2}\left[\psi\left(\frac{14+\sqrt{168}}{4}\right) - \psi\left(\frac{14+\sqrt{168}}{4}\right)\right]$$

Since the digamma terms cancel out, our final answer is simply:
$$\frac{\pi}{4}$$

## Numerical approximation:
$\frac{\pi}{4} \approx 0.7853981634$ rounded to 10 decimal places.

{"answer": "\\frac{\\pi}{4}", "numerical_answer": "0.7853981634"}