To solve the definite integral \(\int\limits_{0}^{2}\frac{x^{-1/2}(2-x)^{-1/2}}{\sqrt{1+x(2-x)}}T_{3}\left(\sqrt{1+x(2-x)}\right)dx\), we need to carefully analyze the integrand and simplify it step by step.

### Step 1: Simplify the integrand

First, let's rewrite the integrand for clarity:
\[ \frac{x^{-1/2}(2-x)^{-1/2}}{\sqrt{1+x(2-x)}} T_{3}\left(\sqrt{1+x(2-x)}\right) \]

Here, \(T_{3}(y)\) is the Chebyshev polynomial of the first kind of degree 3, which is given by:
\[ T_{3}(y) = 4y^3 - 3y \]

Let \( y = \sqrt{1 + x(2 - x)} \). Then:
\[ T_{3}(y) = 4y^3 - 3y \]

Substitute \( y \) back into the integrand:
\[ \frac{x^{-1/2}(2-x)^{-1/2}}{\sqrt{1+x(2-x)}} (4y^3 - 3y) \]

Since \( y = \sqrt{1 + x(2 - x)} \), we have:
\[ y^2 = 1 + x(2 - x) \]
\[ y = \sqrt{1 + x(2 - x)} \]

Thus, the integrand becomes:
\[ \frac{x^{-1/2}(2-x)^{-1/2}}{y} (4y^3 - 3y) \]

Simplify the expression:
\[ \frac{x^{-1/2}(2-x)^{-1/2}}{y} \cdot 4y^3 - \frac{x^{-1/2}(2-x)^{-1/2}}{y} \cdot 3y \]
\[ = 4x^{-1/2}(2-x)^{-1/2} y^2 - 3x^{-1/2}(2-x)^{-1/2} \]

Since \( y^2 = 1 + x(2 - x) \), we have:
\[ 4x^{-1/2}(2-x)^{-1/2} (1 + x(2 - x)) - 3x^{-1/2}(2-x)^{-1/2} \]

### Step 2: Integrate the simplified expression

Now, we need to integrate:
\[ \int_{0}^{2} \left[ 4x^{-1/2}(2-x)^{-1/2} (1 + x(2 - x)) - 3x^{-1/2}(2-x)^{-1/2} \right] dx \]

This can be split into two integrals:
\[ 4 \int_{0}^{2} x^{-1/2}(2-x)^{-1/2} (1 + x(2 - x)) \, dx - 3 \int_{0}^{2} x^{-1/2}(2-x)^{-1/2} \, dx \]

Let's denote these integrals as \( I_1 \) and \( I_2 \):
\[ I_1 = \int_{0}^{2} x^{-1/2}(2-x)^{-1/2} (1 + x(2 - x)) \, dx \]
\[ I_2 = \int_{0}^{2} x^{-1/2}(2-x)^{-1/2} \, dx \]

### Step 3: Evaluate \( I_2 \)

The integral \( I_2 \) is a standard form:
\[ I_2 = \int_{0}^{2} x^{-1/2}(2-x)^{-1/2} \, dx \]

Using the substitution \( x = 2 \sin^2 \theta \), we get:
\[ dx = 4 \sin \theta \cos \theta \, d\theta \]
\[ x^{-1/2} = \frac{1}{\sqrt{2} \sin \theta} \]
\[ (2 - x)^{-1/2} = \frac{1}{\sqrt{2} \cos \theta} \]

Thus:
\[ I_2 = \int_{0}^{\pi/2} \frac{1}{\sqrt{2} \sin \theta} \cdot \frac{1}{\sqrt{2} \cos \theta} \cdot 4 \sin \theta \cos \theta \, d\theta \]
\[ = \int_{0}^{\pi/2} 2 \, d\theta \]
\[ = 2 \left[ \theta \right]_{0}^{\pi/2} \]
\[ = 2 \cdot \frac{\pi}{2} \]
\[ = \pi \]

### Step 4: Evaluate \( I_1 \)

For \( I_1 \), we need to integrate:
\[ I_1 = \int_{0}^{2} x^{-1/2}(2-x)^{-1/2} (1 + x(2 - x)) \, dx \]

Using the same substitution \( x = 2 \sin^2 \theta \):
\[ 1 + x(2 - x) = 1 + 2 \sin^2 \theta (2 - 2 \sin^2 \theta) \]
\[ = 1 + 4 \sin^2 \theta \cos^2 \theta \]
\[ = 1 + \sin^2 2\theta \]

Thus:
\[ I_1 = \int_{0}^{\pi/2} \frac{1}{\sqrt{2} \sin \theta} \cdot \frac{1}{\sqrt{2} \cos \theta} \cdot 4 \sin \theta \cos \theta (1 + \sin^2 2\theta) \, d\theta \]
\[ = \int_{0}^{\pi/2} 2 (1 + \sin^2 2\theta) \, d\theta \]
\[ = 2 \int_{0}^{\pi/2} 1 \, d\theta + 2 \int_{0}^{\pi/2} \sin^2 2\theta \, d\theta \]
\[ = 2 \cdot \frac{\pi}{2} + 2 \cdot \frac{\pi}{4} \]
\[ = \pi + \frac{\pi}{2} \]
\[ = \frac{3\pi}{2} \]

### Step 5: Combine the results

Now, we combine \( I_1 \) and \( I_2 \):
\[ 4I_1 - 3I_2 = 4 \cdot \frac{3\pi}{2} - 3 \cdot \pi \]
\[ = 6\pi - 3\pi \]
\[ = 3\pi \]

### Step 6: Numerical approximation

The numerical approximation of \( 3\pi \) is:
\[ 3 \times 3.141592653589793 \approx 9.424777960769379 \]

### Final Answer

The final answer in the required JSON format is:
```json
{"answer": "3\\pi", "numerical_answer": "9.4247779608"}
```