

To solve the definite integral \(\int_{0}^{2} x^{-1/2}(2 - x)^{-1/2} \cos\left(\sqrt{x(2 - x)}\right) \, dx\), we proceed with the following steps:

### Step 1: Simplify the integrand using substitution
First, rewrite \(x(2 - x)\) by completing the square:
\[
x(2 - x) = 2x - x^2 = 1 - (x - 1)^2.
\]
Let \(x - 1 = \sin\theta\), so \(x = 1 + \sin\theta\). Then:
- When \(x = 0\), \(\sin\theta = -1\) (so \(\theta = -\pi/2\)).
- When \(x = 2\), \(\sin\theta = 1\) (so \(\theta = \pi/2\)).
- \(dx = \cos\theta \, d\theta\).
- \(x(2 - x) = 1 - \sin^2\theta = \cos^2\theta\), so \(\sqrt{x(2 - x)} = \cos\theta\) (since \(\cos\theta \geq 0\) for \(\theta \in [-\pi/2, \pi/2]\)).

### Step 2: Substitute into the integral
The integrand becomes:
\[
x^{-1/2}(2 - x)^{-1/2} = \left[x(2 - x)\right]^{-1/2} = \left[\cos^2\theta\right]^{-1/2} = \frac{1}{\cos\theta}.
\]
Thus, the integral transforms to:
\[
\int_{-\pi/2}^{\pi/2} \frac{1}{\cos\theta} \cdot \cos(\cos\theta) \cdot \cos\theta \, d\theta = \int_{-\pi/2}^{\pi/2} \cos(\cos\theta) \, d\theta.
\]

### Step 3: Exploit symmetry and Bessel function identity
Since \(\cos(\cos\theta)\) is even in \(\theta\), the integral simplifies to:
\[
2 \int_{0}^{\pi/2} \cos(\cos\theta) \, d\theta.
\]
Using the integral representation of the Bessel function \(J_0(z)\):
\[
J_0(z) = \frac{2}{\pi} \int_{0}^{\pi/2} \cos(z \cos\theta) \, d\theta,
\]
we set \(z = 1\) to get:
\[
\int_{0}^{\pi/2} \cos(\cos\theta) \, d\theta = \frac{\pi}{2} J_0(1).
\]
Thus, the original integral becomes:
\[
2 \cdot \frac{\pi}{2} J_0(1) = \pi J_0(1).
\]

### Step 4: Numerical approximation
The Bessel function \(J_0(1) \approx 0.7651976865579665\). Multiplying by \(\pi\) gives:
\[
\pi J_0(1) \approx 3.141592653589793 \cdot 0.7651976865579665 \approx 2.4048255576.
\]

### Final Answer
The exact answer is \(\pi J_0(1)\), and the numerical approximation is \(2.4048255576\).

{"answer": "\(\pi J_0(1)\)", "numerical_answer": "2.4048255576"}