<think>
Okay, so I need to compute the definite integral of cos(x)cos(3x)cos(5x) from 0 to π. Hmm, let's see. I remember that when dealing with products of trigonometric functions, product-to-sum formulas can be really helpful. Maybe I can simplify the product of these cosines into a sum of individual cosine terms. Let me recall the product-to-sum identities.

The product of two cosines can be converted using the formula: cos A cos B = [cos(A+B) + cos(A-B)] / 2. But here we have three cosines multiplied together. So maybe I can first combine two of them and then apply the identity again to the result with the third cosine.

Let me start by taking the first two cosines: cos(x)cos(3x). Applying the product-to-sum formula here:

cos(x)cos(3x) = [cos(x + 3x) + cos(x - 3x)] / 2 = [cos(4x) + cos(-2x)] / 2. But cos(-2x) is the same as cos(2x), so this simplifies to [cos(4x) + cos(2x)] / 2.

Now, the original integral becomes the integral from 0 to π of [cos(4x) + cos(2x)] / 2 * cos(5x) dx. Let me factor out the 1/2:

(1/2) ∫₀^π [cos(4x) + cos(2x)] cos(5x) dx.

Now, I need to distribute cos(5x) over the sum inside the integral:

(1/2) [∫₀^π cos(4x)cos(5x) dx + ∫₀^π cos(2x)cos(5x) dx].

Again, each of these integrals involves the product of two cosines. Let's apply the product-to-sum formula again to each integral.

First integral: cos(4x)cos(5x) = [cos(4x + 5x) + cos(4x - 5x)] / 2 = [cos(9x) + cos(-x)] / 2. Since cos(-x) = cos(x), this becomes [cos(9x) + cos(x)] / 2.

Second integral: cos(2x)cos(5x) = [cos(2x + 5x) + cos(2x - 5x)] / 2 = [cos(7x) + cos(-3x)] / 2. Again, cos(-3x) = cos(3x), so this is [cos(7x) + cos(3x)] / 2.

Substituting these back into the integrals:

(1/2) [ ∫₀^π [cos(9x) + cos(x)] / 2 dx + ∫₀^π [cos(7x) + cos(3x)] / 2 dx ]

Factor out the 1/2 from each integral:

(1/2) * [ (1/2) ∫₀^π [cos(9x) + cos(x)] dx + (1/2) ∫₀^π [cos(7x) + cos(3x)] dx ]

Combine the factors of 1/2:

(1/2)*(1/2 + 1/2) = (1/2)*(1) = 1/4. Wait, no. Wait, let me check that again:

Wait, the expression is (1/2) multiplied by [ (1/2)(Integral) + (1/2)(Integral) ]

So that's (1/2)*(1/2)(Integral1 + Integral2) = (1/4)(Integral1 + Integral2)

Wait, no. Let me re-express:

Original expression after substitution:

(1/2) [ (1/2) [∫cos9x + cosx dx] + (1/2) [∫cos7x + cos3x dx] ]

So that's (1/2) * (1/2)(A + B) + (1/2)(C + D) )

Wait, actually, the first term is (1/2) times [ (1/2)(Integral1) + (1/2)(Integral2) ]

So that's (1/2)*(1/2)(Integral1 + Integral2) = (1/4)(Integral1 + Integral2)

But Integral1 is ∫cos9x + cosx dx from 0 to π, and Integral2 is ∫cos7x + cos3x dx from 0 to π.

So combining them, the entire integral becomes:

(1/4) [ ∫₀^π (cos9x + cosx + cos7x + cos3x) dx ]

So now, we can split this into four separate integrals:

(1/4) [ ∫₀^π cos9x dx + ∫₀^π cosx dx + ∫₀^π cos7x dx + ∫₀^π cos3x dx ]

Now, let's compute each of these integrals individually.

The integral of cos(kx) dx is (1/k) sin(kx) + C. So evaluating each from 0 to π:

For ∫₀^π cos(kx) dx = [sin(kπ)/k - sin(0)/k] = [sin(kπ)/k - 0] = sin(kπ)/k.

But sin(kπ) is zero for any integer k. Because sin(nπ) = 0 when n is an integer. So all these integrals will be zero?

Wait, but wait. Let me check each term:

1. ∫₀^π cos9x dx = [sin(9x)/9] from 0 to π = (sin(9π)/9 - sin(0)/9) = (0 - 0)/9 = 0.

2. ∫₀^π cosx dx = [sinx] from 0 to π = sinπ - sin0 = 0 - 0 = 0.

3. ∫₀^π cos7x dx = [sin7x/7] from 0 to π = (sin7π/7 - 0) = 0.

4. ∫₀^π cos3x dx = [sin3x/3] from 0 to π = (sin3π/3 - 0) = 0.

So all four integrals are zero. Therefore, the entire expression is (1/4)(0 + 0 + 0 + 0) = 0.

Wait, so the integral is zero? That seems too straightforward. Let me verify if I made a mistake in the steps.

Wait, let's check the process again. The original integral is ∫cosx cos3x cos5x dx from 0 to π. Then, using product-to-sum formulas step by step, we broke it down into integrals of cos9x, cosx, cos7x, cos3x, each of which integrates to zero over 0 to π. Therefore, the entire sum is zero, so the integral is zero. Hmm.

But maybe I should check with another method. Alternatively, perhaps using orthogonality of cosine functions over the interval [0, π]. The integral of cos(nx)cos(mx) over 0 to π is zero unless n = m, but here we have products of three cosines. Wait, but after expanding, we have individual terms, each of which is integrated over 0 to π. Since each term is cos(kx) where k is an integer, and integrating from 0 to π gives zero. So yes, the integral is zero.

Alternatively, maybe there's a symmetry consideration. The function cos(x)cos(3x)cos(5x) might be an odd function over some interval, but the interval here is from 0 to π. Let me check if the function is symmetric or antisymmetric around π/2. Let's substitute x with π - t. Let x = π - t, then dx = -dt. When x=0, t=π; when x=π, t=0. So the integral becomes ∫ from π to 0 of cos(π - t)cos(3(π - t))cos(5(π - t)) (-dt) = ∫₀^π cos(π - t)cos(3π - 3t)cos(5π -5t) dt.

But cos(π - t) = -cos t, cos(3π -3t) = -cos(3t), and cos(5π -5t) = -cos(5t). So the product becomes (-cos t)(-cos3t)(-cos5t) = -cos t cos3t cos5t. Therefore, the integral becomes ∫₀^π -cos t cos3t cos5t dt = -∫₀^π cos t cos3t cos5t dt. Let me call the original integral I. Then, this substitution shows that I = -I, which implies that I = 0. Therefore, the integral is zero. So this symmetry argument also gives the same result. Therefore, the integral is indeed zero.

So both methods confirm that the integral is zero. Therefore, the exact answer is 0, and the numerical approximation is also 0.0000000000.

But let me check with a simple numerical approximation. Let's compute the integral numerically. For example, using a calculator or approximate method. Let's take some sample points. For example, at x=0, the integrand is cos0 cos0 cos0 = 1*1*1=1. At x=π/2, cos(π/2)=0, so the integrand is 0. At x=π, cosπ = -1, cos3π = -1, cos5π = -1, so the product is (-1)(-1)(-1) = -1. But integrating from 0 to π, the function is symmetric in a way that positive and negative areas cancel out. But according to the analytical solution, the integral is zero. Let me check with a simple numerical approximation. Let's approximate the integral using the trapezoidal rule with a few intervals. For example, take n=2 intervals. The points are 0, π/2, π. The function values at these points are f(0)=1, f(π/2)=0, f(π)=-1. The trapezoidal approximation would be (π/2)/2 * [f(0) + 2f(π/2) + f(π)] = (π/4)[1 + 0 + (-1)] = (π/4)(0) = 0. Hmm, that's zero. If I take more points, say n=4. Let's see: x=0, π/4, π/2, 3π/4, π. Compute f at each point:

f(0) = 1*1*1=1

f(π/4) = cos(π/4)cos(3π/4)cos(5π/4) = (√2/2)(-√2/2)(-√2/2) = (√2/2)(√2/2)(-√2/2) = ( (2/4) )*(-√2/2) = (1/2)*(-√2/2) = -√2/4 ≈ -0.3535

f(π/2) = 0 as before.

f(3π/4) = cos(3π/4)cos(9π/4)cos(15π/4). Let's compute each:

cos(3π/4) = -√2/2

cos(9π/4) = cos(π/4) = √2/2

cos(15π/4) = cos(7π/4) = √2/2

So product: (-√2/2)(√2/2)(√2/2) = (-2/4)(√2/2) = (-1/2)(√2/2) = -√2/4 ≈ -0.3535

f(π) = -1 as before.

So the trapezoidal approximation with n=4 would be (π/4)/2 [f(0) + 2f(π/4) + 2f(π/2) + 2f(3π/4) + f(π)] = (π/8)[1 + 2*(-0.3535) + 0 + 2*(-0.3535) + (-1)] = (π/8)[1 - 0.707 - 0.707 -1] = (π/8)[-1.414] ≈ (0.3927)(-1.414) ≈ -0.555. But this contradicts the analytical result. Wait, but this is a rough approximation. The trapezoidal rule with n=4 is not very accurate here. Let's try with a larger n. Alternatively, use Simpson's rule. For Simpson's rule with n=2 (which requires even number of intervals), but with n=2, Simpson's rule is (π/3)[f(0) + 4f(π/2) + f(π)] = (π/3)[1 + 0 + (-1)] = 0. So Simpson's rule with n=2 gives zero. But with n=4, Simpson's rule would be (π/12)[f(0) + 4f(π/4) + 2f(π/2) + 4f(3π/4) + f(π)] = (π/12)[1 + 4*(-0.3535) + 0 + 4*(-0.3535) + (-1)] = (π/12)[1 -1.414 -1.414 -1] = (π/12)[-2.828] ≈ (0.2618)(-2.828) ≈ -0.740. Hmm, this is not zero. But according to the analytical solution, the integral is zero. So why the discrepancy? Because the function is oscillatory, and the numerical methods with few intervals are not capturing the cancellations. So perhaps with higher n, the numerical integral approaches zero. Let's try with n=1000 intervals. But since I can't compute that manually, I need to trust the analytical result here. Since both the product-to-sum approach and the symmetry argument give zero, the integral must be zero. Therefore, the exact answer is 0, and the approximation is 0.0000000000.
</think>

{"answer": "0", "numerical_answer": "0.0000000000"}