Let's solve the integral:
\[
\int_{-4}^4 |x^3 - x| \, dx
\]

### Step 1: Find where \( x^3 - x = 0 \)

\[
x^3 - x = x(x^2 - 1) = x(x - 1)(x + 1) = 0
\]
So the roots are at \( x = -1, 0, 1 \).

### Step 2: Break the integral into intervals based on sign change

Check the sign of \( x^3 - x \) in each interval:

- For \( x \in [-4, -1) \):

    At \( x = -2 \):
    \[
    (-2)^3 - (-2) = -8 + 2 = -6 < 0
    \]
    So \( x^3 - x < 0 \)

- For \( x \in (-1, 0) \):

    At \( x = -0.5 \):
    \[
    (-0.5)^3 - (-0.5) = -0.125 + 0.5 = 0.375 > 0
    \]
    So \( x^3 - x > 0 \)

- For \( x \in (0, 1) \):

    At \( x = 0.5 \):
    \[
    (0.5)^3 - 0.5 = 0.125 - 0.5 = -0.375 < 0
    \]
    So \( x^3 - x < 0 \)

- For \( x \in (1, 4] \):

    At \( x = 2 \):
    \[
    8 - 2 = 6 > 0
    \]
    So \( x^3 - x > 0 \)

So the sign of \( x^3 - x \) is:
- Negative on \( [-4, -1] \) and \( [0, 1] \)
- Positive on \( [-1, 0] \) and \( [1, 4] \)

### Step 3: Split the integral

\[
\int_{-4}^4 |x^3 - x| dx = \int_{-4}^{-1} -(x^3 - x) dx + \int_{-1}^{0} (x^3 - x) dx + \int_{0}^{1} -(x^3 - x) dx + \int_{1}^{4} (x^3 - x) dx
\]

\[
= \int_{-4}^{-1} (-x^3 + x) dx + \int_{-1}^{0} (x^3 - x) dx + \int_{0}^{1} (-x^3 + x) dx + \int_{1}^{4} (x^3 - x) dx
\]

### Step 4: Calculate the indefinite integral

\[
\int (x^3 - x) dx = \frac{x^4}{4} - \frac{x^2}{2} + C
\]
\[
\int (-x^3 + x) dx = -\frac{x^4}{4} + \frac{x^2}{2} + C
\]

### Step 5: Compute each term

#### (a) \(\displaystyle \int_{-4}^{-1} (-x^3 + x) dx \)
\[
= \left. \left( -\frac{x^4}{4} + \frac{x^2}{2} \right) \right|_{-4}^{-1}
\]
At \( x = -1 \):
\[
-\frac{(-1)^4}{4} + \frac{(-1)^2}{2} = -\frac{1}{4} + \frac{1}{2} = \frac{1}{4}
\]
At \( x = -4 \):
\[
-\frac{(-4)^4}{4} + \frac{(-4)^2}{2} = -\frac{256}{4} + \frac{16}{2} = -64 + 8 = -56
\]
So, the value is
\[
\frac{1}{4} - (-56) = \frac{1}{4} + 56 = \frac{225}{4}
\]

#### (b) \(\displaystyle \int_{-1}^{0} (x^3 - x) dx \)
\[
= \left. \left( \frac{x^4}{4} - \frac{x^2}{2} \right) \right|_{-1}^0
\]
At \( x = 0 \): \( 0 \)
At \( x = -1 \):
\[
\frac{(-1)^4}{4} - \frac{(-1)^2}{2} = \frac{1}{4} - \frac{1}{2} = -\frac{1}{4}
\]
So, the value is
\[
0 - \left(-\frac{1}{4}\right) = \frac{1}{4}
\]

#### (c) \(\displaystyle \int_{0}^{1} (-x^3 + x) dx \)
\[
= \left. \left( -\frac{x^4}{4} + \frac{x^2}{2} \right) \right|_{0}^{1}
\]
At \( x = 1 \):
\[
-\frac{1}{4} + \frac{1}{2} = \frac{1}{4}
\]
At \( x = 0 \): \( 0 \)
So, the value is
\[
\frac{1}{4} - 0 = \frac{1}{4}
\]

#### (d) \(\displaystyle \int_{1}^{4} (x^3 - x) dx \)
\[
= \left. \left( \frac{x^4}{4} - \frac{x^2}{2} \right) \right|_{1}^{4}
\]
At \( x = 4 \):
\[
\frac{256}{4} - \frac{16}{2} = 64 - 8 = 56
\]
At \( x = 1 \):
\[
\frac{1}{4} - \frac{1}{2} = -\frac{1}{4}
\]
So, the value is
\[
56 - \left(-\frac{1}{4}\right) = 56 + \frac{1}{4} = \frac{225}{4}
\]

### Step 6: Add all terms

Combine:
\[
I = \frac{225}{4} + \frac{1}{4} + \frac{1}{4} + \frac{225}{4}
= \frac{225 + 1 + 1 + 225}{4}
= \frac{452}{4}
= 113
\]

### Step 7: Numerical approximation

\[
113.0000000000
\]

### Step 8: Output in JSON format

```json
{"answer": "\\int_{-4}^4 \\lvert x^3-x\\rvert dx = 113", "numerical_answer": "113.0000000000"}
```