

To solve the definite integral \(\int_{-1}^{0}5\left(x^{6}+x\right)^{4}\:\mathrm{d}x\), we follow these steps:

### Step 1: Expand the integrand
First, expand \(\left(x^6 + x\right)^4\) using the binomial theorem:
\[
\left(x^6 + x\right)^4 = \sum_{k=0}^{4} \binom{4}{k} (x^6)^{4-k} x^k
\]
Calculating each term:
- \(k=0\): \(\binom{4}{0}(x^6)^4 = x^{24}\)
- \(k=1\): \(\binom{4}{1}(x^6)^3 x = 4x^{19}\)
- \(k=2\): \(\binom{4}{2}(x^6)^2 x^2 = 6x^{14}\)
- \(k=3\): \(\binom{4}{3}(x^6) x^3 = 4x^9\)
- \(k=4\): \(\binom{4}{4}x^4 = x^4\)

Thus, \(\left(x^6 + x\right)^4 = x^{24} + 4x^{19} + 6x^{14} + 4x^9 + x^4\).

### Step 2: Multiply by 5 and integrate term-by-term
The integrand becomes \(5\left(x^{24} + 4x^{19} + 6x^{14} + 4x^9 + x^4\right)\). We integrate term-by-term:
\[
\int 5\left(x^{24} + 4x^{19} + 6x^{14} + 4x^9 + x^4\right) \, dx
\]
Integrating each term:
- \(\int 5x^{24} \, dx = 5 \cdot \frac{x^{25}}{25} = \frac{x^{25}}{5}\)
- \(\int 20x^{19} \, dx = 20 \cdot \frac{x^{20}}{20} = x^{20}\)
- \(\int 30x^{14} \, dx = 30 \cdot \frac{x^{15}}{15} = 2x^{15}\)
- \(\int 20x^9 \, dx = 20 \cdot \frac{x^{10}}{10} = 2x^{10}\)
- \(\int 5x^4 \, dx = 5 \cdot \frac{x^5}{5} = x^5\)

Combining these, the antiderivative \(F(x)\) is:
\[
F(x) = \frac{x^{25}}{5} + x^{20} + 2x^{15} + 2x^{10} + x^5
\]

### Step 3: Evaluate the definite integral
We evaluate \(F(x)\) from \(-1\) to \(0\):
\[
\int_{-1}^{0} 5\left(x^6 + x\right)^4 \, dx = F(0) - F(-1)
\]

- At \(x=0\): \(F(0) = 0 + 0 + 0 + 0 + 0 = 0\)
- At \(x=-1\): 
\[
F(-1) = \frac{(-1)^{25}}{5} + (-1)^{20} + 2(-1)^{15} + 2(-1)^{10} + (-1)^5
\]
Simplifying each term:
\[
\frac{-1}{5} + 1 + 2(-1) + 2(1) + (-1) = -\frac{1}{5} + 1 - 2 + 2 - 1 = -\frac{1}{5}
\]

Thus, the integral is:
\[
F(0) - F(-1) = 0 - \left(-\frac{1}{5}\right) = \frac{1}{5}
\]

### Numerical Approximation
The exact value is \(\frac{1}{5}\), which is \(0.2\) when rounded to 10 decimal places.

{"answer": "\(\frac{1}{5}\)", "numerical_answer": "0.2000000000"}