Let's denote the integral as  
\[ I = \int_{0}^{1} \arccos(x) \arctan(x)\, dx \]

### Step 1: Start with Symmetries and Substitutions

Let’s try the substitution \( x = \cos \theta \), with \( dx = -\sin \theta \, d\theta \), and as \( x \) goes from 0 to 1:
- When \( x = 0, \theta = \arccos(0) = \frac{\pi}{2} \)
- When \( x = 1, \theta = \arccos(1) = 0 \)

Hence, the bounds invert:
\[
I = \int_{x=0}^{x=1} \arccos(x) \arctan(x) dx = \int_{\theta = \frac{\pi}{2}}^{0} \theta \arctan(\cos\theta) \cdot (-\sin\theta)\, d\theta
\]
This is:
\[
I = \int_{0}^{\frac{\pi}{2}} \theta \arctan(\cos\theta) \sin\theta\, d\theta
\]

### Step 2: Advance by Expanding \(\arctan(\cos\theta)\)

Let's write \(\arctan(\cos\theta)\) as:
\[
\arctan(\cos\theta) = \int_0^{\cos\theta} \frac{dt}{1+t^2}
\]
But instead, we can use integration by parts on the original integral.

Let’s try integrating by parts on the original \( x \)-variable integral:
Let \( u = \arccos(x) \), \( dv = \arctan(x) dx \).

- \( du = -\frac{1}{\sqrt{1-x^2}} dx \)
- \( v \): to find \( v \), integrate \(\arctan x\):

\[
\int \arctan x dx = x \arctan x - \frac{1}{2} \ln(1 + x^2)
\]

So, \( v = x \arctan x - \frac{1}{2} \ln(1 + x^2) \).

Applying integration by parts:
\[
\int u\, dv = uv - \int v\, du
\]
\[
I = \left[ \arccos(x) (x \arctan x - \frac{1}{2} \ln(1 + x^2)) \right]_{x=0}^{x=1} + \int_{0}^{1} \left(x \arctan x - \frac{1}{2} \ln(1 + x^2)\right) \frac{dx}{\sqrt{1-x^2}}
\]

### Step 3: Evaluate the Boundary Terms

- When \( x=1 \): \(\arccos(1) = 0\), \(1 \arctan 1 = 1 \cdot \frac{\pi}{4} = \frac{\pi}{4}\), \(\ln(1 + 1^2) = \ln 2\)

So at \( x=1 \):
\[
\arccos(1) \left[1 \arctan 1 - \frac{1}{2} \ln 2 \right] = 0
\]

- When \( x=0 \): \(\arccos(0) = \frac{\pi}{2}\), \(0 \cdot \arctan 0 = 0\), \(\ln(1+0^2) = 0\):

\[
\arccos(0) \left[0 - 0\right] = 0
\]

Thus, the boundary term vanishes, and we have:
\[
I = \int_0^1 \left[ x \arctan x - \frac{1}{2} \ln(1 + x^2) \right] \frac{dx}{\sqrt{1 - x^2}}
\]

Let’s split the integral:
\[
I = \int_0^1 \frac{x \arctan x}{\sqrt{1-x^2}} dx - \frac{1}{2} \int_0^1 \frac{\ln(1 + x^2)}{\sqrt{1-x^2}} dx
\]

Let’s denote:
- \( I_1 = \int_0^1 \frac{x \arctan x}{\sqrt{1-x^2}} dx \)
- \( I_2 = \int_0^1 \frac{\ln(1 + x^2)}{\sqrt{1-x^2}} dx \)

### Step 4: Compute \( I_1 \)

Use substitution: \( x = \sin\theta \), where \( \theta \in [0, \pi/2] \)
- \( dx = \cos\theta d\theta \)
- \( \sqrt{1-x^2} = \cos \theta \)

Then:
\[
I_1 = \int_{x=0}^{x=1} \frac{x \arctan x}{\sqrt{1-x^2}} dx = \int_{\theta=0}^{\pi/2} \frac{\sin\theta \arctan(\sin\theta)}{\cos\theta}\cos\theta d\theta
= \int_0^{\pi/2} \sin\theta \arctan (\sin\theta) d\theta
\]

### Step 5: Compute \( I_2 \)

With the same substitution:
\[
I_2 = \int_{0}^{1} \frac{\ln(1 + x^2)}{\sqrt{1-x^2}} dx = \int_{\theta=0}^{\pi/2} \frac{\ln (1+\sin^2\theta)}{\cos\theta} \cos\theta d\theta = \int_0^{\pi/2} \ln (1 + \sin^2\theta) d\theta
\]

### Now, the answer is:
\[
I = \int_0^{\pi/2} \left[ \sin\theta \arctan(\sin\theta) - \frac{1}{2} \ln(1 + \sin^2\theta) \right] d\theta
\]

### Step 6: Reduce or Express in Terms of Known Constants

Let’s try to express \( I \) in terms of elementary or standard constants.

**First term:** 
\[
I_a = \int_0^{\pi/2} \sin\theta \arctan ( \sin\theta ) d\theta
\]

**Second term:**  
\[
I_b = \int_0^{\pi/2} \ln (1 + \sin^2\theta ) d\theta
\]

#### \( I_b \) is a known integral:

\[
\int_0^{\pi/2} \ln ( 1 + a \sin^2 \theta ) d\theta = \frac{\pi}{2} \ln \left( \frac{1 + \sqrt{1+a}}{2} \right), \quad \text{for } a > -1 
\]

For \( a = 1 \):
\[
I_b = \frac{\pi}{2} \ln \left( \frac{1 + \sqrt{2}}{2} \right)
\]

#### For \( I_a \):

Let's expand \(\arctan \sin\theta\) as a Taylor series and try, but it may be best to leave it as is or write it as an integral. Alternatively, let's try integrating by parts.

Let \( u = \arctan (\sin\theta),\ dv = \sin\theta d\theta \).
- \( du = \frac{\cos\theta}{1 + \sin^2\theta} d\theta \)
- \( v = -\cos\theta \)

Then,
\[
I_a = \int_0^{\pi/2} \arctan(\sin\theta) \sin\theta d\theta
= \left[ - \arctan(\sin\theta) \cos\theta \right]_0^{\pi/2}
+ \int_0^{\pi/2} \cos\theta \cdot \frac{\cos\theta}{1+\sin^2\theta} d\theta
\]

Evaluate the boundary term:

At \(\theta = 0\): \(\arctan(0) = 0, \cos 0 = 1\) ⇒ \(0\)

At \(\theta = \frac{\pi}{2}\): \(\sin \frac{\pi}{2} = 1\), \(\arctan(1) = \frac{\pi}{4}\), \(\cos \frac{\pi}{2} = 0\) ⇒ \(0\)

Boundary term is 0.

So,
\[
I_a = \int_0^{\pi/2} \frac{\cos^2\theta}{1 + \sin^2\theta} d\theta
\]
But,
\(
\cos^2 \theta = 1 - \sin^2\theta
\)

So,
\[
I_a = \int_0^{\pi/2} \frac{1-\sin^2\theta}{1 + \sin^2\theta} d\theta = \int_0^{\pi/2} \frac{1}{1+\sin^2\theta} d\theta - \int_0^{\pi/2} \frac{\sin^2\theta}{1+\sin^2\theta} d\theta
\]

But \(
\frac{\sin^2\theta}{1+\sin^2\theta} = 1 - \frac{1}{1+\sin^2\theta}
\), so:

\[
\int_0^{\pi/2} \frac{\sin^2\theta}{1+\sin^2\theta} d\theta = \int_0^{\pi/2} d\theta - \int_0^{\pi/2} \frac{1}{1+\sin^2\theta} d\theta = \frac{\pi}{2} - \int_0^{\pi/2} \frac{1}{1+\sin^2\theta} d\theta
\]

So,
\[
I_a = \int_0^{\pi/2} \frac{1}{1+\sin^2\theta} d\theta - \left(\frac{\pi}{2} - \int_0^{\pi/2} \frac{1}{1+\sin^2\theta} d\theta \right) = 2\int_0^{\pi/2} \frac{1}{1+\sin^2\theta} d\theta - \frac{\pi}{2}
\]

Thus,

\[
I = \left[2\int_0^{\pi/2} \frac{1}{1+\sin^2\theta} d\theta - \frac{\pi}{2}\right] - \frac{1}{2} \cdot \frac{\pi}{2} \ln \left( \frac{1+\sqrt{2}}{2} \right)
\]

Or

\[
I = 2\int_0^{\pi/2} \frac{d\theta}{1+\sin^2\theta} - \frac{\pi}{2} - \frac{\pi}{4} \ln \left( \frac{1+\sqrt{2}}{2} \right)
\]

### Step 7: Evaluate \(\int_0^{\pi/2} \frac{d\theta}{1+\sin^2\theta}\)

Let’s evaluate \( J = \int_0^{\pi/2} \frac{d\theta}{1+\sin^2\theta} \).

This integral is a standard form, and is related to the complete elliptic integral of the first kind.

Use the table:

\[
\int_0^{\pi/2} \frac{d\theta}{a + b \sin^2\theta} = \frac{\pi}{2\sqrt{a(a+b)}}
\]
for \( a > 0, a+b > 0 \).

In our case, \( a = 1, b = 1 \), so

\[
J = \int_0^{\pi/2} \frac{d\theta}{1+\sin^2\theta} = \frac{\pi}{2\sqrt{1\times2}} = \frac{\pi}{2\sqrt{2}}
\]

### Step 8: Assemble the Answer

So,

\[
I = 2 \times \frac{\pi}{2\sqrt{2}} - \frac{\pi}{2} - \frac{\pi}{4} \ln \left( \frac{1+\sqrt{2}}{2} \right)
\]

\[
I = \frac{\pi}{\sqrt{2}} - \frac{\pi}{2} - \frac{\pi}{4} \ln \left( \frac{1+\sqrt{2}}{2} \right)
\]

This is the exact answer.

---

### Step 9: Numerical Evaluation

First, compute each term:

- \(\pi \approx 3.1415926535\)
- \(\sqrt{2} \approx 1.4142135624\)
- \(\frac{1+\sqrt{2}}{2} \approx \frac{1 + 1.4142135624}{2} \approx \frac{2.4142135624}{2} = 1.2071067812\)
- \(\ln(1.2071067812) \approx 0.188324797\)

Now, 
- \(\frac{\pi}{\sqrt{2}} \approx 3.1415926535 / 1.4142135624 \approx 2.2214414691\)
- \(\frac{\pi}{2} \approx 1.5707963268\)
- \(\frac{\pi}{4} \approx 0.7853981634\)

Thus:

\[
I \approx 2.2214414691 - 1.5707963268 - 0.7853981634 \cdot 0.188324797
\]
\[
0.7853981634 \cdot 0.188324797 \approx 0.1478031300
\]

\[
I \approx 2.2214414691 - 1.5707963268 - 0.1478031300
\]
\[
I \approx 2.2214414691 - 1.7185994568 = 0.5028420123
\]

Rounded to 10 decimal places:  
\[
I \approx 0.5028420123
\]

---

### Final JSON Output

```json
{"answer": "\\frac{\\pi}{\\sqrt{2}} - \\frac{\\pi}{2} - \\frac{\\pi}{4} \\ln\\left(\\frac{1+\\sqrt{2}}{2}\\right)", "numerical_answer": "0.5028420123"}
```