# Computing $\int_0^1(x-1)^2(x+1)^2(x^2+1)^2(x^4+1)^2\text{ dx}$

Let's work through this definite integral step by step.

## Step 1: Expand the integrand

The integrand is: $(x-1)^2(x+1)^2(x^2+1)^2(x^4+1)^2$

First, I'll compute the products:
$(x-1)^2(x+1)^2 = (x^2-2x+1)(x^2+2x+1) = x^4+2x^3+x^2-2x^3-4x^2-2x+x^2+2x+1 = x^4-2x^2+1$

So $(x-1)^2(x+1)^2 = x^4-2x^2+1$

Next, $(x^4-2x^2+1)(x^2+1)^2 = (x^4-2x^2+1)(x^4+2x^2+1) = x^8+2x^6+x^4-2x^6-4x^4-2x^2+x^4+2x^2+1 = x^8-2x^4+1$

So $(x-1)^2(x+1)^2(x^2+1)^2 = x^8-2x^4+1$

Finally, $(x^8-2x^4+1)(x^4+1)^2 = (x^8-2x^4+1)(x^8+2x^4+1) = x^{16}+2x^{12}+x^8-2x^{12}-4x^8-2x^4+x^8+2x^4+1 = x^{16}-2x^8+1$

Therefore, our integrand simplifies to:
$(x-1)^2(x+1)^2(x^2+1)^2(x^4+1)^2 = x^{16}-2x^8+1$

## Step 2: Integrate each term

$\int_0^1 (x^{16}-2x^8+1) dx = \int_0^1 x^{16} dx - 2\int_0^1 x^8 dx + \int_0^1 1 dx$

$\int_0^1 x^{16} dx = \left[\frac{x^{17}}{17}\right]_0^1 = \frac{1}{17} - 0 = \frac{1}{17}$

$\int_0^1 x^8 dx = \left[\frac{x^9}{9}\right]_0^1 = \frac{1}{9} - 0 = \frac{1}{9}$

$\int_0^1 1 dx = [x]_0^1 = 1 - 0 = 1$

## Step 3: Combine the results

$\int_0^1 (x^{16}-2x^8+1) dx = \frac{1}{17} - 2\left(\frac{1}{9}\right) + 1 = \frac{1}{17} - \frac{2}{9} + 1$

Let's find a common denominator for these fractions:
$\frac{1}{17} - \frac{2}{9} + 1 = \frac{9}{153} - \frac{34}{153} + \frac{153}{153} = \frac{9-34+153}{153} = \frac{128}{153}$

## Step 4: Numerical approximation

$\frac{128}{153} \approx 0.8366013072$

Therefore, the definite integral equals $\frac{128}{153}$, which is approximately $0.8366013072$ rounded to 10 decimal places.

{"answer": "\\frac{128}{153}", "numerical_answer": "0.8366013072"}