<think>
Okay, let's tackle this integral step by step. The problem is to compute the definite integral from 0 to 2 of x^(-1/2) multiplied by the Hermite polynomial H₃ evaluated at the fourth root of x(2 - x). So, the integral is ∫₀² x^{-1/2} H₃(√[4]{x(2 - x)}) dx. 

First, I need to recall what the Hermite polynomial H₃ looks like. Hermite polynomials are a set of orthogonal polynomials. The third Hermite polynomial H₃(y) is given by H₃(y) = 8y³ - 12y. Let me confirm that. Yes, the standard definition for physicists (since there's also a probabilists' version) is H₃(y) = 8y³ - 12y. So, substituting y with the fourth root of x(2 - x), we have H₃(√[4]{x(2 - x)}) = 8(√[4]{x(2 - x)})³ - 12√[4]{x(2 - x)}.

So the integral becomes ∫₀² x^{-1/2} [8(x(2 - x))^{3/4} - 12(x(2 - x))^{1/4}] dx. Let's factor out the constants: 8∫₀² x^{-1/2} (x(2 - x))^{3/4} dx - 12∫₀² x^{-1/2} (x(2 - x))^{1/4} dx.

Simplify the exponents inside each integral. For the first term: x^{-1/2} * (x(2 - x))^{3/4} = x^{-1/2} * x^{3/4} (2 - x)^{3/4} = x^{(-1/2 + 3/4)} (2 - x)^{3/4} = x^{1/4} (2 - x)^{3/4}. Similarly, the second term: x^{-1/2} * (x(2 - x))^{1/4} = x^{-1/2} * x^{1/4} (2 - x)^{1/4} = x^{-1/4} (2 - x)^{1/4}.

So now the integral is 8∫₀² x^{1/4} (2 - x)^{3/4} dx - 12∫₀² x^{-1/4} (2 - x)^{1/4} dx. Wait, the second term's coefficient is -12, so it's -12 times the integral.

These integrals look like Beta functions. The Beta function is defined as B(a, b) = ∫₀¹ t^{a-1} (1 - t)^{b-1} dt, and it's related to the Gamma function via B(a, b) = Γ(a)Γ(b)/Γ(a + b). To express our integrals in terms of the Beta function, we need to perform a substitution to match the limits of integration from 0 to 1. Let's consider a substitution for the first integral: let t = x/2, so x = 2t, dx = 2dt. Then when x=0, t=0; x=2, t=1. Substituting into the first integral:

8∫₀¹ (2t)^{1/4} (2 - 2t)^{3/4} * 2 dt = 8 * 2^{1/4} * 2^{3/4} * 2 ∫₀¹ t^{1/4} (1 - t)^{3/4} dt. Let's compute the exponents: 2^{1/4} * 2^{3/4} = 2^{(1/4 + 3/4)} = 2^1 = 2. Then multiply by the 2 from dx: 2 * 2 = 4. So the first integral becomes 8 * 4 ∫₀¹ t^{1/4} (1 - t)^{3/4} dt = 32 * B(5/4, 7/4).

Similarly, for the second integral: -12∫₀² x^{-1/4} (2 - x)^{1/4} dx. Let's do the same substitution: x = 2t, dx = 2dt. Then:

-12 * ∫₀¹ (2t)^{-1/4} (2 - 2t)^{1/4} * 2 dt = -12 * 2^{-1/4} * 2^{1/4} * 2 ∫₀¹ t^{-1/4} (1 - t)^{1/4} dt. The exponents on 2: 2^{-1/4 + 1/4} = 2^0 = 1. Then multiply by 2: 2. So this becomes -12 * 2 ∫₀¹ t^{-1/4} (1 - t)^{1/4} dt = -24 * B(3/4, 5/4).

Now, we need to compute these Beta functions. Let's recall that B(a, b) = Γ(a)Γ(b)/Γ(a + b). So for the first term: B(5/4, 7/4) = Γ(5/4)Γ(7/4)/Γ(3). Since Γ(3) = 2! = 2. Similarly, B(3/4, 5/4) = Γ(3/4)Γ(5/4)/Γ(2) = Γ(3/4)Γ(5/4)/1! = Γ(3/4)Γ(5/4).

But Γ(5/4) can be expressed in terms of Γ(1/4) using the property Γ(z + 1) = zΓ(z). So Γ(5/4) = (1/4)Γ(1/4), and Γ(7/4) = (3/4)Γ(3/4). Similarly, Γ(3/4) is just Γ(3/4), and Γ(5/4) is (1/4)Γ(1/4). 

But this might get complicated. Alternatively, we can use the reflection formula or other Gamma function properties. However, perhaps there's a way to relate these Beta functions to each other. Let's compute each term step by step.

First, compute B(5/4, 7/4):

Γ(5/4)Γ(7/4)/Γ(3) = [Γ(5/4)Γ(7/4)] / 2.

Similarly, B(3/4, 5/4) = Γ(3/4)Γ(5/4)/Γ(2) = Γ(3/4)Γ(5/4)/1.

But Γ(7/4) = (3/4)Γ(3/4), so substituting into the first Beta function:

[Γ(5/4) * (3/4)Γ(3/4)] / 2 = (3/8) Γ(5/4)Γ(3/4).

Similarly, the second Beta function is Γ(3/4)Γ(5/4).

So putting it all together:

First integral term: 32 * (3/8) Γ(5/4)Γ(3/4) = 12 Γ(5/4)Γ(3/4).

Second integral term: -24 * Γ(3/4)Γ(5/4).

So combining both terms: 12 Γ(5/4)Γ(3/4) - 24 Γ(3/4)Γ(5/4) = (12 - 24) Γ(3/4)Γ(5/4) = -12 Γ(3/4)Γ(5/4).

Hmm, that's interesting. Wait, but that would mean the entire integral simplifies to -12 Γ(3/4)Γ(5/4). But that seems a bit odd. Let me check the coefficients again.

First term: 8 * 4 ∫₀¹ t^{1/4} (1 - t)^{3/4} dt = 32 * B(5/4, 7/4) = 32 * [Γ(5/4)Γ(7/4)/Γ(3)].

Γ(3) is 2, so 32 * [Γ(5/4)Γ(7/4)/2] = 16 Γ(5/4)Γ(7/4).

But Γ(7/4) = (3/4)Γ(3/4), so 16 Γ(5/4)*(3/4)Γ(3/4) = 16*(3/4) Γ(5/4)Γ(3/4) = 12 Γ(5/4)Γ(3/4).

Second term: -24 * B(3/4, 5/4) = -24 [Γ(3/4)Γ(5/4)/Γ(2)] = -24 Γ(3/4)Γ(5/4)/1 = -24 Γ(3/4)Γ(5/4).

So total integral is 12 Γ(3/4)Γ(5/4) -24 Γ(3/4)Γ(5/4) = -12 Γ(3/4)Γ(5/4).

But Γ(3/4)Γ(5/4) can be simplified using the reflection formula? Wait, Γ(3/4) and Γ(5/4) are related. Alternatively, using the property Γ(z)Γ(1 - z) = π / sin(π z). But 3/4 and 1/4/4? Let's see:

Γ(3/4)Γ(1 - 3/4) = Γ(3/4)Γ(1/4) = π / sin(3π/4) = π / (√2/2) = π√2.

But we have Γ(5/4) = Γ(1/4 + 1) = (1/4)Γ(1/4). So Γ(5/4) = (1/4)Γ(1/4). Similarly, Γ(3/4) is as is.

So Γ(3/4)Γ(5/4) = Γ(3/4)*(1/4)Γ(1/4) = (1/4) Γ(3/4)Γ(1/4) = (1/4) * π√2, from the reflection formula above. Because Γ(3/4)Γ(1/4) = π / sin(π/4) = π / (√2/2) = 2π/√2 = π√2. So Γ(3/4)Γ(1/4) = π√2. Therefore, Γ(3/4)Γ(5/4) = (1/4) * π√2.

Therefore, the integral becomes -12 * (1/4) π√2 = -3 π√2.

Wait, but that's a negative result? Let me check the steps again. The integral was from 0 to 2 of x^{-1/2} H₃(√[4]{x(2 - x)}) dx. The Hermite polynomial H₃ is 8y³ -12y. The substitution led to integrals that resulted in -12 Γ(3/4)Γ(5/4), which then simplified to -3π√2. But integrating over 0 to 2, and the integrand... Wait, let's check if the integrand is positive or negative.

Wait, x is between 0 and 2. The term x(2 - x) is between 0 and 1 (since it's a quadratic with maximum at x=1, value 1*1=1). So the fourth root of x(2 - x) is between 0 and 1. Then H₃(y) = 8y³ -12y. For y in (0,1), let's see: at y=0, H₃(0) = -0. At y=1, H₃(1) = 8 -12 = -4. So H₃ is negative in this interval. Then x^{-1/2} is positive. So the integrand is negative over (0,2). So the integral should be negative, which matches our result of -3π√2. But let's check the numerical approximation.

But let's compute the numerical value. π is approximately 3.1415926536, √2 is about 1.4142135624. So -3 * π * √2 ≈ -3 * 3.1415926536 * 1.4142135624 ≈ -3 * 4.442882908 ≈ -13.328648724. Let's see if that's the case.

But wait, maybe I made a mistake in the sign. Let's check the steps. The Hermite polynomial H₃(y) = 8y³ -12y. Then substituting into the integral, we have 8y³ -12y. Then when we split the integral into two parts: 8 times the integral of x^{-1/2} y³ dx minus 12 times the integral of x^{-1/2} y dx. Then after substitutions, the first integral became 12 Γ(3/4)Γ(5/4) and the second term -24 Γ(3/4)Γ(5/4). So 12 -24 = -12. Then Γ(3/4)Γ(5/4) = (1/4) Γ(3/4)Γ(1/4) = (1/4) * π√2. So -12 * (1/4) π√2 = -3 π√2. So the exact answer is -3π√2. But the integral of a negative function over the interval should be negative, which matches. But let's check if the steps are correct.

Alternatively, maybe there's a mistake in the substitution. Let me verify the substitution steps again.

For the first integral: ∫₀² x^{1/4} (2 - x)^{3/4} dx. Let t = x/2, so x = 2t, dx = 2dt. Then x^{1/4} = (2t)^{1/4} = 2^{1/4} t^{1/4}, and (2 - x)^{3/4} = (2 - 2t)^{3/4} = (2(1 - t))^{3/4} = 2^{3/4} (1 - t)^{3/4}. Then the integral becomes ∫₀¹ 2^{1/4} t^{1/4} * 2^{3/4} (1 - t)^{3/4} * 2 dt = 2^{1/4 + 3/4 +1} ∫₀¹ t^{1/4} (1 - t)^{3/4} dt. The exponents: 1/4 + 3/4 = 1, plus 1 from the dx gives 2. So 2^2 = 4. So 4 * B(5/4, 7/4). Then multiplied by 8 from the original integral's coefficient: 8 * 4 * B(5/4,7/4) = 32 B(5/4,7/4). Then, as before, B(5/4,7/4) = Γ(5/4)Γ(7/4)/Γ(3) = Γ(5/4)*(3/4 Γ(3/4))/2. So 32 * (3/8) Γ(5/4)Γ(3/4) = 12 Γ(5/4)Γ(3/4). That's correct.

For the second integral: ∫₀² x^{-1/4} (2 - x)^{1/4} dx. Substituting x=2t, dx=2dt. Then x^{-1/4} = (2t)^{-1/4} = 2^{-1/4} t^{-1/4}, (2 - x)^{1/4} = (2(1 - t))^{1/4} = 2^{1/4} (1 - t)^{1/4}. So the integral becomes ∫₀¹ 2^{-1/4} t^{-1/4} * 2^{1/4} (1 - t)^{1/4} * 2 dt. The exponents on 2: -1/4 +1/4 =0, plus 1 from dx gives 2^1=2. So 2 ∫₀¹ t^{-1/4} (1 - t)^{1/4} dt = 2 B(3/4,5/4). Then the coefficient is -12, so -12 * 2 B(3/4,5/4) = -24 B(3/4,5/4). Then B(3/4,5/4) = Γ(3/4)Γ(5/4)/Γ(2) = Γ(3/4)Γ(5/4). So total is -24 Γ(3/4)Γ(5/4).

Combining both terms: 12 Γ(5/4)Γ(3/4) -24 Γ(3/4)Γ(5/4) = -12 Γ(3/4)Γ(5/4). Then using Γ(5/4) = (1/4)Γ(1/4), so Γ(3/4)Γ(5/4) = (1/4) Γ(3/4)Γ(1/4). And Γ(3/4)Γ(1/4) = π / sin(π/4) = π / (√2/2) = π√2. Therefore, Γ(3/4)Γ(5/4) = (1/4) π√2. So the integral becomes -12 * (1/4) π√2 = -3 π√2. 

But wait, the integral is negative. However, when I think about the integrand, x^{-1/2} is positive, and H₃(y) is negative in the interval (since y is between 0 and 1, and H₃(y) =8y³ -12y. At y=0, it's 0 -0 =0? Wait, no. Wait, H₃(0) = 0 -12*0 =0. Wait, but for y in (0,1), let's take y=0.5. Then H₃(0.5) =8*(0.125) -12*(0.5) =1 -6= -5. So negative. So the integrand is negative over (0,2), so the integral should be negative. So -3π√2 is correct.

But let's check the numerical value. π is approximately 3.141592653589793, √2 is approximately 1.4142135623730951. So multiplying: 3 * π * √2 ≈ -3 * 3.141592653589793 * 1.4142135623730951 ≈ -3 * 4.442882908158169 ≈ -13.328648724474507. Rounded to 10 decimal places, that's approximately -13.3286487245.

But wait, the problem says to compute the definite integral from 0 to 2. But the answer is negative. However, let's check if there's a mistake in the substitution or in the Hermite polynomial. Let me confirm H₃(y). The physicists' Hermite polynomials are given by H₀(y)=1, H₁(y)=2y, H₂(y)=4y²-2, H₃(y)=8y³ -12y. Yes, that's correct. So H₃(y) is indeed 8y³ -12y.

Another check: when x approaches 0, x^{-1/2} behaves like 1/√x, which is integrable at 0 since the integral of x^{-1/2} converges. Similarly, at x=2, (2 - x) is approaching 0, but (2 - x)^{3/4} and (2 - x)^{1/4} are also integrable. So the integral is convergent.

Therefore, the exact answer is -3π√2, and the numerical approximation is approximately -13.3286487245. However, let me verify this with a numerical integration to check.

Alternatively, perhaps there's a substitution that can simplify the integral. Let's consider substituting t = √[4]{x(2 - x)}. Let y = √[4]{x(2 - x)}. Then y⁴ = x(2 - x). Let's see if we can express x in terms of y. However, this might complicate things. Alternatively, another substitution.

Let me try substituting x = 2 sin²θ. Then when x=0, θ=0; x=2, θ=π/2. Then dx = 4 sinθ cosθ dθ. Then x(2 - x) = 2 sin²θ * 2 cos²θ = 4 sin²θ cos²θ = (2 sinθ cosθ)^2 = sin²(2θ). So the fourth root of x(2 - x) is √[4]{sin²(2θ)} = √|sin(2θ)|. But since θ is between 0 and π/2, sin(2θ) is non-negative, so it's √(sin(2θ)) = (sin(2θ))^{1/2}.

But H₃(y) =8y³ -12y. So H₃(√[4]{x(2 - x)}) =8 (sin(2θ))^{3/2} -12 (sin(2θ))^{1/2}.

Also, x^{-1/2} = (2 sin²θ)^{-1/2} = (1/√2) (sinθ)^{-1}.

Putting it all together, the integral becomes:

∫₀^{π/2} (1/√2)(sinθ)^{-1} [8 (sin2θ)^{3/2} -12 (sin2θ)^{1/2}] *4 sinθ cosθ dθ.

Simplify term by term:

First, constants: (1/√2) *4 = 4/√2 = 2√2.

Then, sinθ^{-1} * sinθ = 1. So the integral becomes:

2√2 ∫₀^{π/2} [8 (sin2θ)^{3/2} -12 (sin2θ)^{1/2}] cosθ dθ.

Factor out 4:

2√2 [8 ∫₀^{π/2} (sin2θ)^{3/2} cosθ dθ -12 ∫₀^{π/2} (sin2θ)^{1/2} cosθ dθ ].

But 8*2√2 = 16√2 and -12*2√2 = -24√2. Wait, no. Wait, the 2√2 is multiplied by the entire bracket. So:

2√2 *8 ∫ ... - 2√2 *12 ∫ ... = 16√2 ∫ ... -24√2 ∫ ... 

But let's compute each integral separately.

Let me compute the first integral: ∫₀^{π/2} (sin2θ)^{3/2} cosθ dθ.

Let’s make a substitution. Let u = θ. Hmm, perhaps substitute t = sinθ. Let’s try substitution t = sinθ. Then dt = cosθ dθ. When θ=0, t=0; θ=π/2, t=1. Then the integral becomes ∫₀¹ (sin2θ)^{3/2} dt. But sin2θ = 2 sinθ cosθ = 2 t √(1 - t²). So (sin2θ)^{3/2} = (2 t √(1 - t²))^{3/2} = 2^{3/2} t^{3/2} (1 - t²)^{3/4}. So the integral becomes 2^{3/2} ∫₀¹ t^{3/2} (1 - t²)^{3/4} dt.

This looks like a Beta function. Let’s make substitution z = t². Then t = z^{1/2}, dt = (1/2) z^{-1/2} dz. When t=0, z=0; t=1, z=1. The integral becomes 2^{3/2} ∫₀¹ (z^{1/2})^{3/2} (1 - z)^{3/4} * (1/2) z^{-1/2} dz = 2^{3/2} * 1/2 ∫₀¹ z^{3/4 -1/2} (1 - z)^{3/4} dz = 2^{1/2} ∫₀¹ z^{1/4} (1 - z)^{3/4} dz = √2 B(5/4, 7/4).

Similarly, the second integral: ∫₀^{π/2} (sin2θ)^{1/2} cosθ dθ. Using the same substitution t = sinθ, dt = cosθ dθ. Then sin2θ = 2t√(1 - t²), so (sin2θ)^{1/2} = (2t√(1 - t²))^{1/2} = 2^{1/2} t^{1/2} (1 - t²)^{1/4}. The integral becomes ∫₀¹ 2^{1/2} t^{1/2} (1 - t²)^{1/4} dt. Substitute z = t², t = z^{1/2}, dt = (1/2) z^{-1/2} dz. Then:

2^{1/2} ∫₀¹ (z^{1/2})^{1/2} (1 - z)^{1/4} * (1/2) z^{-1/2} dz = 2^{1/2} * 1/2 ∫₀¹ z^{-1/4} (1 - z)^{1/4} dz = 2^{-1/2} B(3/4, 5/4).

So putting it all together:

First integral: 16√2 * √2 B(5/4,7/4) = 16*2 B(5/4,7/4) = 32 B(5/4,7/4).

Second integral: -24√2 * 2^{-1/2} B(3/4,5/4) = -24√2 / √2 B(3/4,5/4) = -24 B(3/4,5/4).

Which brings us back to the same expressions as before. So the same result: -3π√2. Therefore, the analytical solution is confirmed.

Now, the numerical approximation. As calculated earlier, -3π√2 ≈ -3 * 3.141592653589793 * 1.4142135623730951 ≈ -13.328648724474507. Rounded to 10 decimal places, that's -13.3286487245.

But let me verify this with a calculator. Let's value:

π ≈ 3.1415926536

√2 ≈ 1.4142135624

Multiply them: 3.1415926536 * 1.4142135624 ≈ 4.442882908158169

Then multiply by 3: 4.442882908158169 * 3 ≈ 13.328648724474507

So with the negative sign, it's -13.3286487245.

Therefore, the exact answer is -3π√2, and the numerical approximation is approximately -13.3286487245.
</think>

{"answer": "-3\\sqrt{2}\\pi", "numerical_answer": "-13.3286487245"}