Let's calculate the integral:
\[
I = \int_0^{\frac{\pi}{2}} x \ln(\sin x) \, dx
\]

**Step 1: Use a Fourier series for \(\ln(\sin x)\).**

Recall the Fourier expansion:
\[
\ln(\sin x) = -\ln 2 - \sum_{k=1}^\infty \frac{\cos(2 k x)}{k}
\]

Substitute this into the integral:
\[
I = \int_0^{\frac{\pi}{2}} x \left( -\ln 2 - \sum_{k=1}^\infty \frac{\cos(2 k x)}{k} \right) dx
\]
\[
= -\ln 2 \int_0^{\frac{\pi}{2}} x \, dx - \sum_{k=1}^\infty \frac{1}{k} \int_0^{\frac{\pi}{2}} x \cos(2k x) dx
\]

The first integral:
\[
\int_0^{\frac{\pi}{2}} x \, dx = \left. \frac{x^2}{2} \right|_0^{\frac{\pi}{2}} = \frac{1}{2} \left(\frac{\pi}{2}\right)^2 = \frac{\pi^2}{8}
\]
So,
\[
-\ln 2 \cdot \frac{\pi^2}{8}
\]

**Step 2: Compute the second integral.**

Letâ€™s compute
\[
J_k = \int_0^{\frac{\pi}{2}} x \cos(2k x) dx
\]

Integrate by parts:
Let \(u = x,\ dv = \cos(2k x) dx\)  
So \(du = dx,\ v = \frac{\sin(2k x)}{2k}\)

\[
= x \cdot \frac{\sin(2k x)}{2k}\Big|_0^{\frac{\pi}{2}} - \int_0^{\frac{\pi}{2}} \frac{\sin(2k x)}{2k} dx
\]

Compute boundaries:
\[
x = 0: \sin(0) = 0; \quad x = \frac{\pi}{2}: \sin(2k \cdot \frac{\pi}{2}) = \sin(k\pi) = 0
\]
So the first term vanishes.

The remaining integral:
\[
-\int_0^{\frac{\pi}{2}} \frac{\sin(2k x)}{2k} dx = -\frac{1}{2k}\int_0^{\frac{\pi}{2}} \sin(2k x) dx
\]

Compute \(\int_0^{\frac{\pi}{2}} \sin(2k x) dx\):

The antiderivative is \(-\frac{\cos(2k x)}{2k}\):

\[
\left[ -\frac{\cos(2k x)}{2k} \right]_0^{\frac{\pi}{2}} = -\frac{\cos(k\pi) - 1}{2k}
\]
So,
\[
J_k = 0 + \frac{1}{2k} \cdot \left(-\frac{\cos(k\pi) - 1}{2k}\right) 
= -\frac{\cos(k\pi) - 1}{4k^2}
\]

Recall \(\cos(k\pi) = (-1)^k\):

So,
\[
J_k = -\frac{(-1)^k - 1}{4k^2}
\]

**Step 3: Substitute back into the sum:**

Recall:
\[
I = -\ln 2 \cdot \frac{\pi^2}{8} - \sum_{k=1}^\infty \frac{1}{k} J_k
\]
\[
= -\frac{\pi^2}{8} \ln 2 - \sum_{k=1}^\infty \frac{1}{k} \left( -\frac{(-1)^k - 1}{4k^2} \right )
\]
\[
= -\frac{\pi^2}{8} \ln 2 + \frac{1}{4} \sum_{k=1}^\infty \frac{(-1)^k - 1}{k^3}
\]

\[
= -\frac{\pi^2}{8} \ln 2 + \frac{1}{4} \left( \sum_{k=1}^\infty \frac{(-1)^k}{k^3} - \sum_{k=1}^\infty \frac{1}{k^3} \right )
\]

Recall:
\[
\sum_{k=1}^\infty \frac{1}{k^s} = \zeta(s)
\]
\[
\sum_{k=1}^\infty \frac{(-1)^k}{k^s} = -\eta(s)
\]
where \(\eta(s) = (1-2^{1-s})\zeta(s)\) is the Dirichlet eta function.

So,
\[
\sum_{k=1}^\infty \frac{(-1)^k}{k^3} = -\eta(3)
\]
So,
\[
I = -\frac{\pi^2}{8} \ln 2 + \frac{1}{4} \left( -\eta(3) - \zeta(3) \right )
\]
\[
= -\frac{\pi^2}{8} \ln 2 - \frac{1}{4} (\eta(3) + \zeta(3))
\]

But,
\[
\eta(3) = (1-2^{-2})\zeta(3) = \left (1-\frac{1}{4} \right ) \zeta(3) = \frac{3}{4}\zeta(3)
\]
So,
\[
\eta(3) + \zeta(3) = \frac{3}{4}\zeta(3) + \zeta(3) = \frac{7}{4}\zeta(3)
\]
Thus,
\[
I = -\frac{\pi^2}{8} \ln 2 - \frac{7}{16} \zeta(3)
\]

**Step 4: Provide a numerical approximation**

- \(\pi^2 \approx 9.8696044011\)
- \(\ln 2 \approx 0.6931471806\)
- \(\zeta(3) \approx 1.2020569032\)

\[
-\frac{\pi^2}{8}\ln 2 \approx -\frac{9.8696044011}{8} \times 0.6931471806 \approx -1.2337005501 \times 0.6931471806 \approx -0.8551808630
\]
\[
-\frac{7}{16}\zeta(3) \approx -0.4375 \times 1.2020569032 \approx -0.5258908951
\]
Final sum:
\[
I \approx -0.8551808630 - 0.5258908951 \approx -1.3810717581
\]

**Final JSON answer:**
```json
{"answer": "-\\frac{\\pi^2}{8} \\ln 2 - \\frac{7}{16}\\zeta(3)", "numerical_answer": "-1.3810717581"}
```