We wish to evaluate

  I = ∫₀² [1/(x(2–x))]·arctan(√(x(2–x))) dx.

A good strategy is to make a substitution that “symmetrizes” the integrand. Notice that

  x(2–x) = 1 – (x–1)².

Thus it is natural to use a sine–substitution. In fact, let

  x = 1 + sin t.

Then when x goes from 0 to 2 the corresponding t-values are:
  • When x = 0: 1 + sin t = 0 ⟹ sin t = –1 ⟹ t = –π/2.
  • When x = 2: 1 + sin t = 2 ⟹ sin t = 1 ⟹ t =  π/2.

Also note:
  dx = cos t dt.

Furthermore, we compute:
  x(2–x) = (1+sin t)(2–(1+sin t)) = (1+sin t)(1–sin t) = 1 – sin²t = cos²t,
so that
  √(x(2–x)) = |cos t| = cos t   (since for t in [–π/2, π/2] we have cos t ≥ 0).

We also have
  x⁻¹(2–x)⁻¹ = 1/[(1+ sin t)(1– sin t)] = 1/(1– sin²t) = 1/cos²t.

Thus the integrand transforms as follows:
  [1/(x(2–x))]·arctan(√(x(2–x))) dx = [1/cos²t]·arctan(cos t)·(cos t dt)
                    = arctan(cos t)/cos t dt.

So the original integral becomes

  I = ∫ₜ₌₋π/2^(π/2) [arctan(cos t)/cos t] dt.

Notice that cos t is an even function and arctan(cos t) is even (since cos(–t)=cos t), so the integrand is even. Hence we can write

  I = 2 ∫₀^(π/2) [arctan(cos t)/cos t] dt.

Define

  J = ∫₀^(π/2) [arctan(cos t)/cos t] dt,
so that I = 2J.

Now, to evaluate J we use a useful representation of the arctan function. For any z we have

  arctan z = ∫₀¹ [z/(1+u²z²)] du.
 
Here, with z = cos t, we get

  arctan(cos t) = ∫₀¹ [cos t/(1+u²cos²t)] du.
 
Substitute this into the integral defining J:
 
  J = ∫₀^(π/2) { [1/cos t] · [∫₀¹ cos t/(1+u²cos²t) du] } dt
    = ∫₀^(π/2) ∫₀¹ [1/(1+u²cos²t)] du dt.
 
Since the integrals are over a product region and everything is nonnegative, we can interchange the order of integration:
 
  J = ∫₀¹ { ∫₀^(π/2) dt/(1+u²cos²t) } du.
 
Now, the inner t–integral is a standard integral. (One often finds the formula in tables or by making a complement substitution t → π/2 – t.) In fact one may show that

  ∫₀^(π/2) dt/(1+u²cos²t) = (π/2)/√(1+u²).

Thus,
 
  J = ∫₀¹ (π/2)/√(1+u²) du = (π/2) ∫₀¹ du/√(1+u²).

The remaining u–integral is elementary:
 
  ∫ du/√(1+u²) = sinh⁻¹ u = ln(u+√(1+u²)).
 
Evaluating from u = 0 to 1 gives
 
  ∫₀¹ du/√(1+u²) = ln(1+√2) – ln(0+1) = ln(1+√2).

Thus,
 
  J = (π/2) ln(1+√2).
 
Recalling that I = 2J, we finally have
 
  I = 2 · (π/2) ln(1+√2) = π ln(1+√2).

For a numerical approximation, we note:
  √2 ≈ 1.4142135624 → 1+√2 ≈ 2.4142135624,
  ln(2.4142135624) ≈ 0.881373,
so that
  π ln(1+√2) ≈ 3.1415926536 × 0.881373 ≈ 2.7689320221.

Thus, the final answer is

  I = π ln(1+√2)  ≈ 2.7689320221

{"answer": "\\pi \\ln\\left(1+\\sqrt{2}\\right)", "numerical_answer": "2.7689320221"}