We wish to evaluate
  I = ∫₆₄⁷²⁹ (x^(1/2))/(x^(1/2) – x^(1/3)) dx.

Step 1. Rewrite the integrand.
Notice that:
  x^(1/2) = x^(1/3)·x^(1/6),
so
  x^(1/2) – x^(1/3) = x^(1/3)(x^(1/6) – 1).
Thus the integrand becomes
  [x^(1/3)·x^(1/6)] / [x^(1/3)(x^(1/6) – 1)] = x^(1/6)/(x^(1/6) – 1).

Step 2. Make the substitution u = x^(1/6). Then:
  x = u⁶  and  dx = 6u⁵ du.
When x = 64, u = 64^(1/6) = 2  (since 64 = 2⁶),
and when x = 729, u = 729^(1/6) = 3  (since 729 = 3⁶).

The integrand becomes:
  x^(1/6)/(x^(1/6) – 1) dx = u/(u – 1)·(6u⁵ du) = 6 u⁶/(u – 1) du.
Thus,
  I = 6 ∫₂³ (u⁶/(u – 1)) du.

Step 3. Divide u⁶ by (u – 1).
Perform polynomial division:
  u⁶/(u – 1) = u⁵ + u⁴ + u³ + u² + u + 1 + 1/(u – 1),
since (u – 1)(u⁵ + u⁴ + u³ + u² + u + 1) = u⁶ – 1.

Thus the integral becomes:
  I = 6 ∫₂³ [u⁵ + u⁴ + u³ + u² + u + 1 + 1/(u – 1)] du.

Step 4. Integrate term‐by‐term.
The indefinite integrals are:
  ∫ u⁵ du = u⁶/6,
  ∫ u⁴ du = u⁵/5,
  ∫ u³ du = u⁴/4,
  ∫ u² du = u³/3,
  ∫ u du = u²/2,
  ∫ 1 du = u,
  ∫ 1/(u – 1) du = ln|u – 1|.
Therefore,
  I = 6 { [u⁶/6 + u⁵/5 + u⁴/4 + u³/3 + u²/2 + u + ln|u – 1|] evaluated from u = 2 to u = 3 }.

Step 5. Evaluate at the bounds.
At u = 3:
  A = 3⁶/6 = 729/6 = 243/2,
  B = 3⁵/5 = 243/5,
  C = 3⁴/4 = 81/4,
  D = 3³/3 = 27/3 = 9,
  E = 3²/2 = 9/2,
  F = 3,
  G = ln(3 – 1) = ln2.
At u = 2:
  A' = 2⁶/6 = 64/6 = 32/3,
  B' = 2⁵/5 = 32/5,
  C' = 2⁴/4 = 16/4 = 4,
  D' = 2³/3 = 8/3,
  E' = 2²/2 = 2,
  F' = 2,
  G' = ln(2 – 1) = ln1 = 0.

Thus the difference F(3) – F(2) is:
  [243/2 – 32/3] + [243/5 – 32/5] + [81/4 – 4] + [9 – 8/3] + [9/2 – 2] + [3 – 2] + [ln2 – 0].

It is best to break the sum into two parts.

First, note that the integration multiplied by 6 gives:
  I = [3⁶ – 2⁶] + 6 { (243/5 – 32/5) + (81/4 – 4) + (9 – 8/3) + (9/2 – 2) + (3 – 2) } + 6 ln2.
Since 3⁶ = 729 and 2⁶ = 64, the term [3⁶ – 2⁶] = 729 – 64 = 665.

Now, compute the remaining bracket:
1) (243/5 – 32/5) = (211/5).
2) (81/4 – 4) = (81/4 – 16/4) = 65/4.
3) (9 – 8/3) = (27/3 – 8/3) = 19/3.
4) (9/2 – 2) = (9/2 – 4/2) = 5/2.
5) (3 – 2) = 1.
Adding the constant terms: 211/5, 65/4, 19/3, 5/2, and 1.

Find a common denominator. The LCM of 5, 4, 3, and 2 is 60.
Convert:
  211/5 = (211×12)/60 = 2532/60,
  65/4 = (65×15)/60 = 975/60,
  19/3 = (19×20)/60 = 380/60,
  5/2 = (5×30)/60 = 150/60,
  1 = 60/60.
Sum = (2532 + 975 + 380 + 150 + 60) / 60 =  (2532 + 975 = 3507; 3507 + 380 = 3887; 3887 + 150 = 4037; 4037 + 60 = 4097) = 4097/60.

Now multiply by 6:
  6 × (4097/60) = 4097/10.

Thus, the full result is:
  I = 665 + (4097/10) + 6 ln2.
Write 665 as (6650/10) so that:
  I = (6650 + 4097)/10 + 6 ln2 = (10747/10) + 6 ln2.

However, note that when we processed the antiderivative the term at u = 3 also contributed the term 243/2 coming from u⁶/6. To keep things completely consistent, we can also integrate term‐by‐term directly from our antiderivative:

The antiderivative is
  F(u) = u⁶/6 + u⁵/5 + u⁴/4 + u³/3 + u²/2 + u + ln|u – 1|.
Then
  I = 6 [F(3) – F(2)].

Compute F(3):
  = 729/6 + 243/5 + 81/4 + 27/3 + 9/2 + 3 + ln2
  = 243/2 + 243/5 + 81/4 + 9 + 9/2 + 3 + ln2.
F(2):
  = 64/6 + 32/5 + 16/4 + 8/3 + 4/2 + 2 + ln1
  = 32/3 + 32/5 + 4 + 8/3 + 2 + 2.
Simplify F(2):
  Combine 32/3 + 8/3 = 40/3 and 2+2 = 4; so F(2) = 40/3 + 32/5 + 4 + 4 = 40/3 + 32/5 + 8.
Thus, F(3) – F(2) equals:
  [243/2 + 243/5 + 81/4 + 9 + 9/2 + 3 + ln2] – [40/3 + 32/5 + 8].

Group like terms:
• 243/5 – 32/5 = 211/5.
• 243/2 + 9/2 = (243 + 9)/2 = 252/2 = 126.
• The constants: 9 + 3 = 12 and then subtract 8 gives 4.
• Remaining term: 81/4 from F(3) and −40/3 from F(2), and + ln2.

So F(3) – F(2) = 126 + 211/5 + 81/4 + 4 – 40/3 + ln2.

Convert the rational numbers with denominator 60:
  126 = 126*(60/60) = 7560/60,
  211/5 = (211×12)/60 = 2532/60,
  81/4 = (81×15)/60 = 1215/60,
  4 = 240/60,
  40/3 = (40×20)/60 = 800/60.
Thus, the combined rational part is:
  (7560 + 2532 + 1215 + 240 – 800) / 60 = (7560 + 2532 = 10092; 10092 + 1215 = 11307; 11307 + 240 = 11547; 11547 – 800 = 10747)/60.
Then,
  F(3) – F(2) = 10747/60 + ln2.
Now multiply by 6:
  I = 6 [10747/60 + ln2] = (10747/10) + 6 ln2.

Thus the final answer is:
  I = (10747 + 60 ln2) / 10.

Step 6. Compute a numerical approximation.
Using ln2 ≈ 0.69314718056:
  60 ln2 ≈ 41.5888308336,
then
  I ≈ (10747 + 41.5888308336)/10 = 10788.5888308336/10 ≈ 1078.8588830834.

So the numerical value rounded to 10 decimal places is 1078.8588830834.

Final answer in JSON format:

{"answer": "\\frac{10747+60\\\\ln(2)}{10}", "numerical_answer": "1078.8588830834"}