To compute the definite integral 

\[
\int_0^1 \frac{e^{\arctan(x)}}{(x^2 + 1)^{3/2}} \, dx,
\]

we proceed with the following steps:

### Step 1: Substitution
Let \( u = \arctan(x) \). Then, the derivative of \( u \) with respect to \( x \) is:

\[
\frac{du}{dx} = \frac{1}{x^2 + 1} \quad \Rightarrow \quad dx = (x^2 + 1) \, du.
\]

When \( x = 0 \), \( u = 0 \), and when \( x = 1 \), \( u = \frac{\pi}{4} \).

### Step 2: Rewrite the Integral in Terms of \( u \)
Substituting \( x = \tan(u) \), we have \( x^2 + 1 = \tan^2(u) + 1 = \sec^2(u) \). Thus, the integrand becomes:

\[
\frac{e^{\arctan(x)}}{(x^2 + 1)^{3/2}} = \frac{e^u}{(\sec^2(u))^{3/2}} = \frac{e^u}{\sec^3(u)} = e^u \cos^3(u).
\]

The integral transforms as:

\[
\int_0^1 \frac{e^{\arctan(x)}}{(x^2 + 1)^{3/2}} \, dx = \int_0^{\pi/4} e^u \cos^3(u) \, du.
\]

### Step 3: Simplify the Integral
We can simplify \( \cos^3(u) \) using the identity:

\[
\cos^3(u) = \frac{3\cos(u) + \cos(3u)}{4}.
\]

Thus, the integral becomes:

\[
\int_0^{\pi/4} e^u \cos^3(u) \, du = \frac{1}{4} \int_0^{\pi/4} e^u (3\cos(u) + \cos(3u)) \, du.
\]

### Step 4: Integrate Using Integration by Parts
We use the standard result for integrals of the form \( \int e^{au} \cos(bu) \, du \):

\[
\int e^{au} \cos(bu) \, du = \frac{e^{au}}{a^2 + b^2} (a \cos(bu) + b \sin(bu)) + C.
\]

Applying this to our integral:

\[
\int e^u \cos(u) \, du = \frac{e^u}{2} (\cos(u) + \sin(u)) + C,
\]

\[
\int e^u \cos(3u) \, du = \frac{e^u}{10} (\cos(3u) + 3 \sin(3u)) + C.
\]

Now, evaluate these from \( 0 \) to \( \pi/4 \):

\[
\left. \frac{e^u}{2} (\cos(u) + \sin(u)) \right|_0^{\pi/4} = \frac{e^{\pi/4}}{2} \left( \cos\left(\frac{\pi}{4}\right) + \sin\left(\frac{\pi}{4}\right) \right) - \frac{1}{2} (1 + 0) = \frac{e^{\pi/4}}{2} \left( \frac{\sqrt{2}}{2} + \frac{\sqrt{2}}{2} \right) - \frac{1}{2} = \frac{e^{\pi/4} \sqrt{2}}{2} - \frac{1}{2},
\]

\[
\left. \frac{e^u}{10} (\cos(3u) + 3 \sin(3u)) \right|_0^{\pi/4} = \frac{e^{\pi/4}}{10} \left( \cos\left(\frac{3\pi}{4}\right) + 3 \sin\left(\frac{3\pi}{4}\right) \right) - \frac{1}{10} (1 + 0) = \frac{e^{\pi/4}}{10} \left( -\frac{\sqrt{2}}{2} + 3 \cdot \frac{\sqrt{2}}{2} \right) - \frac{1}{10} = \frac{e^{\pi/4} \sqrt{2}}{5} - \frac{1}{10}.
\]

Combine these results:

\[
\frac{1}{4} \left( 3 \left( \frac{e^{\pi/4} \sqrt{2}}{2} - \frac{1}{2} \right) + \left( \frac{e^{\pi/4} \sqrt{2}}{5} - \frac{1}{10} \right) \right) = \frac{1}{4} \left( \frac{3e^{\pi/4} \sqrt{2}}{2} + \frac{e^{\pi/4} \sqrt{2}}{5} - \frac{3}{2} - \frac{1}{10} \right).
\]

Simplify the coefficients:

\[
\frac{3}{2} + \frac{1}{5} = \frac{15}{10} + \frac{2}{10} = \frac{17}{10},
\]

\[
\frac{3e^{\pi/4} \sqrt{2}}{2} + \frac{e^{\pi/4} \sqrt{2}}{5} = e^{\pi/4} \sqrt{2} \left( \frac{3}{2} + \frac{1}{5} \right) = e^{\pi/4} \sqrt{2} \cdot \frac{17}{10}.
\]

Thus, the integral evaluates to:

\[
\frac{1}{4} \left( \frac{17 e^{\pi/4} \sqrt{2}}{10} - \frac{17}{10} \right) = \frac{17}{40} \left( e^{\pi/4} \sqrt{2} - 1 \right).
\]

### Step 5: Final Answer
The exact value of the integral is:

\[
\frac{17}{40} \left( \sqrt{2} e^{\pi/4} - 1 \right).
\]

A numerical approximation to 10 decimal places is:

\[
0.7455632325.
\]

### JSON Output
```json
{"answer": "\\frac{17}{40} \\left( \\sqrt{2} e^{\\pi/4} - 1 \\right)", "numerical_answer": "0.7455632325"}
```