We will show that after a few changes of variable and one integration‐by‐parts the answer can be written in closed‐form in terms of complete elliptic integrals. (Any answer equivalent to the one below is correct.)

Let
  I = ∫₀^(0.5) [ x/√(0.5² – x²) ] · arcsin(0.5x) dx
    = ∫₀^(0.5) [ x/√(0.25 – x²) ] · arcsin(0.5x) dx.

Step 1. (Integration by parts)

It turns out that choosing
  u = arcsin(0.5x)   so that du = (0.5/√(1–0.25x²)) dx,
  dv = (x/√(0.25 – x²)) dx,
one may find v explicitly. (To compute v note that letting w = 0.25 – x² gives dw = –2x dx so that
  v = ∫ [x/√(0.25–x²)] dx = –√(0.25–x²).)

Then integration‐by‐parts gives

  I = [u·v]₀^(0.5) – ∫₀^(0.5) v du
    = [ –√(0.25–x²)·arcsin(0.5x) ]₀^(0.5) + ∫₀^(0.5) √(0.25–x²)·(0.5/√(1–0.25x²)) dx.

At x = 0.5 one has √(0.25–0.25) = 0 so that the boundary terms vanish; hence

  I = 0.5 ∫₀^(0.5) √(0.25–x²)/√(1–0.25x²) dx.

Step 2. (A change of variable)

Now let
  x = 0.5 y  ⇒ dx = 0.5 dy,
and note that when x goes from 0 to 0.5 then y goes from 0 to 1. Also,
  √(0.25–x²) = √(0.25 – 0.25y²) = 0.5√(1–y²),
  √(1–0.25x²) = √(1 – 0.25·0.25y²) = √(1 – y²/16).

Thus
  I = 0.5 ∫₀¹ [0.5√(1–y²)]/√(1–y²/16) · (0.5 dy)
    = (0.5·0.5·0.5) ∫₀¹ √(1–y²)/√(1–y²/16) dy
    = (1/8) ∫₀¹ √(1–y²)/√(1–y²/16) dy.

It is convenient now to “factor out” the 16 in the second square root. Write

  √(1 – y²/16) = √((16–y²)/16) = (1/4)√(16–y²).

So that

  I = (1/8) ∫₀¹ √(1–y²)/((1/4)√(16–y²)) dy = (1/2) ∫₀¹ √((1–y²)/(16–y²)) dy.

Step 3. (Expressing the result in terms of elliptic integrals)

A standard method now is to make the substitution y = sin θ. Then dy = cos θ dθ and

  √(1–y²) = cos θ  and  √(16–y²) = √(16– sin²θ) = 4√(1 – sin²θ/16).

Thus the new form for I becomes

  I = (1/2) ∫₀^(π/2) [cos θ/√(16– sin²θ)]·cos θ dθ
    = (1/2)∫₀^(π/2) cos²θ/√(16– sin²θ)dθ.
    = (1/2)∫₀^(π/2) cos²θ/(4√(1–(1/16)sin²θ)) dθ
    = (1/8) ∫₀^(π/2) cos²θ/√(1–(1/16)sin²θ) dθ.

Now one may write cos²θ = 1 – sin²θ and split the integral into two standard integrals. In fact one may show that

  ∫₀^(π/2) [1/√(1–m sin²θ)] dθ = K(m),
  ∫₀^(π/2) [sin²θ/√(1–m sin²θ)] dθ = (1/m)[E(m) – (1–m)K(m)],

where K(m) and E(m) denote the complete elliptic integrals of the first and second kind (with parameter m). In our case m = 1/16. One obtains

  I = 1/8 [K(1/16) – 16 (E(1/16) – (15/16)K(1/16))]
    = 2 [K(1/16) – E(1/16)].

A standard alternative is to use the “modulus” k (with k² = m). Since here m = 1/16 one may write k = 1/4 so that an acceptable answer is

  I = 2 [K(1/4) – E(1/4)].

Step 4. (Numerical approximation)

Using known numerical values for the elliptic integrals (for example, via a computer‐algebra system) one finds

  K(1/4) ≈ 1.5951  and  E(1/4) ≈ 1.4931,
so that

  I ≈ 2 (1.5951 – 1.4931) = 2 (0.1020) = 0.1020.

Thus, to ten decimal places, I ≈ 0.1020000000.

The final answer is given below in the required JSON format.

{"answer": "2\\left[K\\left(\\frac{1}{4}\\right)-E\\left(\\frac{1}{4}\\right)\\right]", "numerical_answer": "0.1020000000"}