Let's proceed step by step.

## 1. Recall the Hermite polynomial \( H_3(x) \):

\[
H_3(x) = 8x^3 - 12x
\]

## 2. Substitute the expression inside \( H_3 \):

\[
H_3(\sqrt{x(2-x)}) = 8[\sqrt{x(2-x)}]^3 - 12\sqrt{x(2-x)} = 8 [x(2-x)]^{3/2} - 12 [x(2-x)]^{1/2}
\]

Therefore,
\[
I = \int_0^2 H_3(\sqrt{x(2-x)}) dx = 8\int_0^2 [x(2-x)]^{3/2} dx - 12\int_0^2 [x(2-x)]^{1/2} dx
\]

Letâ€™s denote:
\[
I_1 = \int_0^2 [x(2-x)]^{3/2} dx
\]
\[
I_2 = \int_0^2 [x(2-x)]^{1/2} dx
\]

So:
\[
I = 8I_1 - 12I_2
\]

---

## 3. Compute \( I_1 \) and \( I_2 \) with a suitable substitution

Let \( x = 2\sin^2\theta \), where as \( x \) goes from 0 to 2, \( \theta \) goes from 0 to \(\frac{\pi}{2}\).

Calculate:

- \( x = 2\sin^2\theta \implies dx = 4\sin\theta\cos\theta d\theta = 2\sin(2\theta)d\theta \)
- \( 2 - x = 2 - 2\sin^2\theta = 2\cos^2\theta \)
- \( x(2-x) = 2\sin^2\theta \cdot 2\cos^2\theta = 4\sin^2\theta\cos^2\theta = 4\sin^2\theta\cos^2\theta \)

### Consider
\[
[x(2-x)]^{n/2} = 2^n [\sin^n\theta \cos^n\theta]
\]
So the \( dx \) brings in \( 2\sin(2\theta)d\theta \).

Let's compute for both \(n = 3\) and \(n = 1\):

---

### For \( I_n = \int_{x=0}^{2} [x(2-x)]^{n/2} dx \):

Change of variables:
- When \( x = 0 \), \( \sin^2\theta = 0 \implies \theta = 0 \).
- When \( x = 2 \), \( \sin^2\theta = 1 \implies \theta = \frac{\pi}{2} \).

So,
\[
I_n = \int_{0}^{\pi/2} [4\sin^2\theta\cos^2\theta]^{n/2} \cdot 2\sin(2\theta) d\theta
\]

\[
4^{n/2} = 2^n \implies
\]
\[
[\sin^2\theta\cos^2\theta]^{n/2} = [\sin\theta\cos\theta]^n
\]
\[
\sin(2\theta) = 2\sin\theta\cos\theta
\]
So combine:
\[
I_n = 2^n \int_0^{\pi/2} [\sin^n\theta \cos^n\theta] \cdot 2\sin(2\theta) d\theta \\
= 2^{n+1} \int_0^{\pi/2} \sin^n\theta \cos^n\theta \cdot \sin(2\theta) d\theta
\]

But,
\[
\sin(2\theta) = 2\sin\theta\cos\theta
\]
So,
\[
I_n = 2^{n+1} \int_0^{\pi/2} \sin^n\theta \cos^n\theta \cdot 2\sin\theta\cos\theta d\theta \\
= 2^{n+2} \int_0^{\pi/2} \sin^{n+1}\theta \cos^{n+1}\theta d\theta
\]

---

### Now, explicit evaluation:
\[
I_n = 2^{n+2} \int_0^{\pi/2} \sin^{n+1}\theta \cos^{n+1}\theta d\theta
\]

Express as a beta function:
\[
\int_0^{\pi/2} \sin^a\theta \cos^b\theta d\theta = \frac{1}{2}B\left(\frac{a+1}{2},\frac{b+1}{2}\right)
\]

So:
\[
I_n = 2^{n+2} \cdot \frac{1}{2} B\left(\frac{n+2}{2}, \frac{n+2}{2}\right) = 2^{n+1} B\left(\frac{n+2}{2}, \frac{n+2}{2}\right)
\]

But \( B(p, q) = \frac{\Gamma(p)\Gamma(q)}{\Gamma(p+q)} \).

---

#### Compute \( I_1 \) and \( I_2 \):

#### For \( I_1: n=3 \)
\[
I_1 = 2^{4} B\left(\frac{4}{2}, \frac{4}{2}\right) = 16 B(2,2)
\]
But \( B(2,2) = \frac{\Gamma(2)^2}{\Gamma(4)} \).
- \( \Gamma(2) = 1 \)
- \( \Gamma(4) = 3! = 6 \)
So,
\[
B(2,2) = \frac{1^2}{6} = \frac{1}{6}
\]
Hence,
\[
I_1 = 16 \cdot \frac{1}{6} = \frac{8}{3}
\]

---

#### For \( I_2: n=1 \)
\[
I_2 = 2^{2} B\left(\frac{2}{2}, \frac{2}{2}\right) = 4 B(1,1)
\]
\( B(1,1) = \frac{\Gamma(1)^2}{\Gamma(2)} = \frac{1}{1} = 1 \)
So,
\[
I_2 = 4 \cdot 1 = 4
\]

---

## 4. Compute the original integral

\[
I = 8I_1 - 12I_2 = 8 \cdot \frac{8}{3} - 12 \cdot 4 = \frac{64}{3} - 48 = \frac{64 - 144}{3} = \frac{-80}{3}
\]

---

## 5. Numerical value

\[
\frac{-80}{3} \approx -26.6666666667
\]

---

## 6. JSON Output

```json
{"answer": "\\frac{-80}{3}", "numerical_answer": "-26.6666666667"}
```