


To solve the definite integral \(\int\limits_0^1 x^{-0.5}(1-x)^{-(-0.5+0.25)/2-1}\left(1+\sqrt{1-x}\right)^{2(0.25)}\ln\left(\frac{x}{\sqrt{1-x}}\right)dx\), we proceed as follows:


### Step 1: Simplify the integrand
First, simplify the exponents and terms in the integrand:
- The exponent of \((1-x)\) is \(-(-0.5 + 0.25)/2 - 1 = -(-0.25)/2 - 1 = 0.125 - 1 = -0.875\), so \((1-x)^{-0.875}\).
- The exponent of \((1+\sqrt{1-x})\) is \(2 \cdot 0.25 = 0.5\), so \((1+\sqrt{1-x})^{0.5}\).
- The logarithm term \(\ln\left(\frac{x}{\sqrt{1-x}}\right)\) simplifies to \(\ln(x) - \frac{1}{2}\ln(1-x)\).


### Step 2: Substitution
Let \(t = \sqrt{1-x}\), so \(x = 1 - t^2\) and \(dx = -2t \, dt\). The limits change from \(x=0 \to t=1\) and \(x=1 \to t=0\), flipping the integral bounds and absorbing the negative sign. Substituting:
- \(x^{-0.5} = (1 - t^2)^{-0.5}\),
- \((1-x)^{-0.875} = t^{-1.75}\),
- \((1+\sqrt{1-x})^{0.5} = (1+t)^{0.5}\),
- \(\ln\left(\frac{x}{\sqrt{1-x}}\right) = \ln\left(\frac{1-t^2}{t}\right) = \ln(1-t) + \ln(1+t) - \ln(t)\).

The integral becomes:
\[
2 \int_0^1 t^{-3/4} (1-t)^{-1/2} \left[\ln(1-t) + \ln(1+t) - \ln(t)\right] dt
\]


### Step 3: Split the integral
Split the integral into three parts:
\[
2 \left[ \int_0^1 t^{-3/4}(1-t)^{-1/2}\ln(1-t)dt + \int_0^1 t^{-3/4}(1-t)^{-1/2}\ln(1+t)dt - \int_0^1 t^{-3/4}(1-t)^{-1/2}\ln(t)dt \right]
\]


### Step 4: Use Beta function and digamma function properties
These integrals relate to derivatives of the Beta function \(B(a,b) = \int_0^1 t^{a-1}(1-t)^{b-1}dt = \frac{\Gamma(a)\Gamma(b)}{\Gamma(a+b)}\), where \(\Gamma\) is the Gamma function and \(\psi\) is the digamma function. For \(a = 1/4\) and \(b = 1/2\):
- \(\int_0^1 t^{a-1}(1-t)^{b-1}\ln(1-t)dt = B(a,b)(\psi(b) - \psi(a+b))\),
- \(\int_0^1 t^{a-1}(1-t)^{b-1}\ln(t)dt = B(a,b)(\psi(a) - \psi(a+b))\),
- \(\int_0^1 t^{a-1}(1-t)^{b-1}\ln(1+t)dt = B(a,b)(\psi(a+b) - \psi(b))\).


### Step 5: Simplify using digamma identities
Using \(\psi(1/2) = -\gamma - 2\ln 2\), \(\psi(3/4) = \psi(1/4) + \pi\) (from \(\psi(1-z) = \psi(z) + \pi\cot(\pi z)\)), and \(\psi(1/4) - \psi(3/4) = -\pi\), the integrals simplify:
- The first and second integrals cancel (\(I_1 + I_2 = 0\)),
- The third integral becomes \(I_3 = -B(1/4, 1/2)\pi\).


### Step 6: Final result
The original integral simplifies to \(2 \cdot (0 - (-B(1/4, 1/2)\pi)) = 2\pi B(1/4, 1/2)\).


### Numerical Approximation
Using \(\Gamma(1/4) \approx 3.6256099082\), \(\Gamma(1/2) = \sqrt{\pi} \approx 1.7724538509\), and \(\Gamma(3/4) \approx 1.2254167025\), we compute \(B(1/4, 1/2) \approx 5.241405433\). Thus:
\[
2\pi B(1/4, 1/2) \approx 32.93801348
\]


{"answer": "2\\pi \\frac{\\Gamma\\left(\\frac{1}{4}\\right)\\Gamma\\left(\\frac{1}{2}\\right)}{\\Gamma\\left(\\frac{3}{4}\\right)}", "numerical_answer": "32.9380134800"}