Let's evaluate the definite integral:
\[
\int_0^{\pi/4}\frac{\tan(x)+2\sec^2(x)+2\tan(x)\sec^2(x)}{\tan(x)+\sec^2(x)}\;dx
\]

---

### Step 1: Simplify the Integrand

Let’s let \( T = \tan(x) \) and \( S = \sec^2(x) \).

The integrand is:
\[
\frac{T + 2S + 2TS}{T + S}
\]

Let’s factor numerator:
\[
T + 2S + 2TS = T + 2S + 2TS = (T + S) + S + 2TS = (T + S) + S(1 + 2T)
\]
But that's not really simpler. Let’s instead factor directly:

\[
T + 2S + 2TS = T + 2TS + 2S = T(1 + 2S) + 2S
\]

Let’s consider polynomial division:

\[
\frac{T + 2S + 2TS}{T + S} 
\]
Let’s write numerator as:
\[
[T + 2TS] + 2S = T(1 + 2S) + 2S
\]
Alternatively, factor \( S \):
\[
T + 2S + 2TS = T + 2TS + 2S = T(1+2S) + 2S
\]
Let’s do polynomial long division or make it explicit.

#### Let’s factor numerator in terms of \( T \):

\[
= \frac{T(1 + 2S) + 2S}{T + S}
\]

Let’s divide:

Let’s try to write as:
\[
= \frac{(T + S) + S + 2TS}{T + S}
= 1 + \frac{S + 2TS}{T + S}
\]
Let’s factor \( S \):
\[
= 1 + \frac{S(1 + 2T)}{T + S}
\]

So the integrand is:
\[
1 + \frac{S(1 + 2T)}{T + S}
\]

Let’s split it further:
Let’s write \( S(1 + 2T) = \sec^2(x)(1 + 2\tan(x)) \).

But before proceeding, let's try to write \( (1 + 2T)/(T + S) \).

Let’s represent everything in sines and cosines:

\(
\tan(x) = \frac{\sin(x)}{\cos(x)},\;
\sec^2(x) = \frac{1}{\cos^2(x)}
\)

So,
\[
\tan(x) + 2\sec^2(x) + 2\tan(x)\sec^2(x)
= \frac{\sin(x)}{\cos(x)} + 2\frac{1}{\cos^2(x)} + 2\frac{\sin(x)}{\cos(x)} \cdot \frac{1}{\cos^2(x)}
\]
\[
= \frac{\sin(x)}{\cos(x)} + \frac{2}{\cos^2(x)} + \frac{2\sin(x)}{\cos^3(x)}
\]

The denominator is \(\tan(x) + \sec^2(x) = \frac{\sin(x)}{\cos(x)} + \frac{1}{\cos^2(x)}\).

Let’s write all terms over a common denominator:
\[
\tan(x) + \sec^2(x) = \frac{\sin(x)\cos(x) + 1}{\cos^2(x)}
\]
So,
\[
\tan(x) + \sec^2(x) = \frac{\sin(x)\cos(x) + 1}{\cos^2(x)}
\]

The numerator:
Let's write all terms over \(\cos^3(x)\):

First term: \(\frac{\sin(x)}{\cos(x)} = \frac{\sin(x)\cos^2(x)}{\cos^3(x)}\)

Second term: \(\frac{2}{\cos^2(x)} = \frac{2\cos(x)}{\cos^3(x)}\)

Third term: \(\frac{2\sin(x)}{\cos^3(x)}\)

So sum:
\[
\frac{\sin(x)\cos^2(x) + 2\cos(x) + 2\sin(x)}{\cos^3(x)}
\]

So the integrand is:
\[
\frac{\sin(x)\cos^2(x) + 2\cos(x) + 2\sin(x)}{\cos^3(x)} 
\Bigg/ 
\frac{\sin(x)\cos(x) + 1}{\cos^2(x)}
\]
Or,
\[
\frac{\sin(x)\cos^2(x) + 2\cos(x) + 2\sin(x)}{\cos^3(x)}
\cdot
\frac{\cos^2(x)}{\sin(x)\cos(x) + 1}
=
\frac{\sin(x)\cos^2(x) + 2\cos(x) + 2\sin(x)}{\cos^3(x)}
\cdot
\frac{\cos^2(x)}{\sin(x)\cos(x) + 1}
\]

Combine numerator:
\[
\frac{[\sin(x)\cos^2(x) + 2\cos(x) + 2\sin(x)] \cdot \cos^2(x)}{\cos^3(x)[\sin(x)\cos(x) + 1]}
\]
\[
= \frac{\sin(x)\cos^4(x) + 2\cos^3(x) + 2\sin(x)\cos^2(x)}{\cos^3(x)[\sin(x)\cos(x) + 1]}
\]

Now, factor \(\cos^2(x)\) out of numerator:
\[
= \frac{\cos^2(x) [\sin(x)\cos^2(x) + 2\cos(x) + 2\sin(x)]}{\cos^3(x)[\sin(x)\cos(x) + 1]}
\]
\[
= \frac{[\sin(x)\cos^2(x) + 2\cos(x) + 2\sin(x)]}{\cos(x)[\sin(x)\cos(x) + 1]}
\]

Let’s write numerator:
\[
\sin(x)\cos^2(x) + 2\cos(x) + 2\sin(x)
= [\sin(x)\cos^2(x) + 2\sin(x)] + 2\cos(x)
= \sin(x)[\cos^2(x) + 2] + 2\cos(x)
\]
\[
= \sin(x)[1 + \cos^2(x)] + 2\cos(x)
\]
But that's probably not simplifying further.

Let’s leave the integrand as:
\[
I = \int_0^{\pi/4} \frac{\sin(x)\cos^2(x) + 2\cos(x) + 2\sin(x)}{\cos(x)[\sin(x)\cos(x) + 1]} dx
\]

Alternatively, factor numerator differently:
\[
\sin(x)\cos^2(x) + 2\cos(x) + 2\sin(x)
= \sin(x)\cos^2(x) + 2\sin(x) + 2\cos(x)
= \sin(x)[\cos^2(x) + 2] + 2\cos(x)
\]
Still, not overly helpful.

Let’s consider substituting \( u = \tan(x) \), \( x \in [0, \pi/4] \Rightarrow u \in [0, 1] \).

Let's try this substitution:

From \( u = \tan x \) we have:
\[
\sin x = \frac{u}{\sqrt{1+u^2}}, \quad \cos x = \frac{1}{\sqrt{1+u^2}}, \quad \sec^2 x = 1 + u^2
\]
Also, \( dx = \frac{du}{1+u^2} \).

---

### Step 2: Substitute with \(u = \tan(x)\)

Let’s rewrite the original numerator and denominator in terms of \(u\):

Original numerator:
\[
\tan(x) + 2\sec^2(x) + 2\tan(x)\sec^2(x)
= u + 2(1 + u^2) + 2u(1+u^2)
\]
Compute \(2u(1+u^2) = 2u + 2u^3\).
So:
\[
u + 2(1 + u^2) + 2u(1 + u^2) = u + 2 + 2u^2 + 2u + 2u^3 = (u + 2u + 2u^2 + 2u^3 + 2)
= (3u + 2u^2 + 2u^3 + 2)
\]
Or, written ordered by descending order:
\[
2u^3 + 2u^2 + 3u + 2
\]

Denominator:
\[
\tan(x) + \sec^2(x) = u + (1 + u^2) = u^2 + u + 1
\]

Also, \( dx = \frac{du}{1+u^2} \).

So, the integrand in terms of \(u\):
\[
\int_{u=0}^{u=1} 
\frac{2u^3 + 2u^2 + 3u + 2}{u^2 + u + 1} \cdot \frac{1}{1+u^2} du
\]

Now, expand numerator:
\[
2u^3 + 2u^2 + 3u + 2
\]
Denominator is \( (u^2 + u + 1)(u^2 + 1) \).

Let’s expand denominator:
\[
(u^2 + u + 1)(u^2 + 1) = u^4 + u^2 + u^3 + u + u^2 + 1 = u^4 + u^3 + 2u^2 + u + 1
\]

So, the definite integral is:
\[
I = \int_{0}^{1} \frac{2u^3 + 2u^2 + 3u + 2}{u^4 + u^3 + 2u^2 + u + 1} du
\]

---

### Step 3: Attempt Partial Fractions

We need to integrate
\[
I = \int_{0}^{1} \frac{2u^3 + 2u^2 + 3u + 2}{u^4 + u^3 + 2u^2 + u + 1} du
\]

Let’s factor denominator if possible. Otherwise, let's try polynomial division.

Check degree: numerator is degree 3, denominator degree 4, so proper rational function.

Let’s try to write numerator as derivative of denominator plus a constant.

Compute derivative of denominator:
\[
f(u) = u^4 + u^3 + 2u^2 + u + 1 \\
f'(u) = 4u^3 + 3u^2 + 4u + 1
\]

Compare numerator:
\[
\text{Num}(u) = 2u^3 + 2u^2 + 3u + 2\\
f'(u) = 4u^3 + 3u^2 + 4u + 1
\]

Now, let's see if Num(u) = A f'(u) + B.

Let’s suppose Num(u) = a f'(u) + b.

Set up:
\[
a(4u^3 + 3u^2 + 4u + 1) + b = 2u^3 + 2u^2 + 3u + 2
\]
Equate coefficients:
- \( u^3: \quad 4a = 2 \implies a = \frac{1}{2} \)
- \( u^2: \quad 3a = 2 \implies a = \frac{2}{3} \)
Oops, inconsistency. So numerator is *not* a multiple of derivative + constant.

Let's try to express numerator as a linear combination:

Suppose:
\[
2u^3 + 2u^2 + 3u + 2
= A \cdot (4u^3 + 3u^2 + 4u + 1 ) + 
B \cdot (u^4 + u^3 + 2u^2 + u + 1 ) + C
\]
But that's complicated.

Alternatively, try substitution: denominator in the form
\[
u^4 + u^3 + 2u^2 + u + 1 = (u^2 + \alpha u + 1)(u^2 + \beta u + 1)
\]
Let's attempt to factor.

Let
\[
(u^2 + a u + 1)(u^2 + b u + 1) = u^4 + (a+b)u^3 + (ab+2)u^2 + (a+b)u + 1
\]
Comparing to given denominator:
\[
u^4 + u^3 + 2u^2 + u + 1
\]
So:
\[
a+b = 1 \\
ab + 2 = 2 \implies ab = 0 \\
\]
So either \(a = 0, b=1\) or \(a=1, b=0\).

Thus,
\[
u^4 + u^3 + 2u^2 + u + 1 = (u^2 + 0\cdot u + 1)(u^2 + 1 \cdot u + 1) = (u^2 + 1)(u^2 + u + 1)
\]
So denominator factors as
\[
(u^2 + 1)(u^2 + u + 1)
\]

Therefore:
\[
I = \int_{0}^{1} \frac{2u^3 + 2u^2 + 3u + 2}{(u^2 + 1)(u^2 + u + 1)} du
\]

---

### Step 4: Partial Fraction Decomposition

Let’s write:
\[
\frac{2u^3 + 2u^2 + 3u + 2}{(u^2 + 1)(u^2 + u + 1)} = \frac{A u + B}{u^2 + 1} + \frac{Cu + D}{u^2 + u + 1}
\]

Multiply both sides by the denominator:
\[
2u^3 + 2u^2 + 3u + 2 = (A u + B)(u^2 + u + 1) + (C u + D)(u^2 + 1)
\]
Expand:

First, \( (A u + B)(u^2 + u + 1) = A u(u^2 + u + 1) + B(u^2 + u + 1) = A u^3 + A u^2 + A u + B u^2 + B u + B \)

Second, \( (C u + D)(u^2 + 1) = C u^3 + C u + D u^2 + D \)

Sum:
\[
2u^3 + 2u^2 + 3u + 2 = \\
(A u^3 + C u^3) 
+ (A u^2 + B u^2 + D u^2) 
+ (A u + B u + C u) 
+ (B + D)
\]
But let's write all out:

- \(u^3: \quad A + C \)
- \(u^2: \quad A + B + D \)
- \(u^1: \quad A + B + C \)
- constants: \(B + D\)

Wait, more carefully:

Expand:
\[
(A u + B)(u^2 + u + 1) = A u^3 + A u^2 + A u + B u^2 + B u + B \\
= A u^3 + (A + B) u^2 + (A + B) u + B
\]
Similarly,
\[
(C u + D)(u^2 + 1) = C u^3 + C u + D u^2 + D \\
= C u^3 + D u^2 + C u + D
\]

Add together:
\[
\text{Sum:}
\]
- \(u^3\): \(A + C\)
- \(u^2\): \(A + B + D\)
- \(u^1\): \(A + B + C\)
- constant: \(B + D\)

But wait, above I had:
- \(u^3\): \(A + C\)
- \(u^2\): \(A + B + D\)
- \(u^1\): \(A + B + C\)
- \(u^0\): \(B + D\)

But let's double-check the \(u^1\) terms:
- From \((A u + B)(u^2 + u + 1)\): \(A u\), from \(A u \cdot 1\), and \(A u \cdot u = A u^2\), \(A u \cdot u^2 = A u^3\); \(B \cdot u = B u\).
- So \(A u^3\), \(A u^2\), \(A u\), \(B u^2\), \(B u\), \(B\).

So \(u^3\): \(A\).
\(u^2\): \(A + B\).
\(u\): \(A + B\) [?]. Let's check: from above, \(A u\) and \(B u\) = \((A + B)u\).

Similarly, from \((C u + D)(u^2 + 1)\): \(C u^3\), \(D u^2\), \(C u\), \(D\).

Sum:
- \(u^3\): \(A + C\)
- \(u^2\): \(A + B + D\)
- \(u\): \(A + B + C\)
- constant: \(B + D\)

But let's be careful—correct way is collect powers:

- \(u^3\): \(A u^3\) from first, \(C u^3\) from second → \(A + C\)
- \(u^2\): \(A u^2\) and \(B u^2\) from first, \(D u^2\) from second → \(A + B + D\)
- \(u\): \(A u\) and \(B u\) from first, \(C u\) from second → \(A + B + C\)
- constant: \(B\) from first, \(D\) from second → \(B + D\)

But wait, the expansion goes as:

\((A u + B)(u^2 + u + 1) = A u^3 + A u^2 + A u + B u^2 + B u + B\).

So \(u^3\): \(A\)
\(u^2\): \(A + B\)
\(u^1\): \(A + B\)
\(u^0\): \(B\)

From \((C u + D)(u^2 + 1)\): \(C u^3\), \(D u^2\), \(C u\), \(D\).

Now sum:
- \(u^3\): \(A + C\)
- \(u^2\): \(A + B + D\)
- \(u^1\): \(A + B + C\)
- constant: \(B + D\)

But in previous expansion, we had \(A u\), and \(B u\).
Thus, the total coefficient of \(u\) is \(A u + B u + C u = (A + B + C) u\).

Wait, that's off. Let's break it down.

Expand term by term:

First, expand \((A u + B)(u^2 + u + 1)\):

\[
A u \cdot u^2 = A u^3 \\
A u \cdot u = A u^2 \\
A u \cdot 1 = A u \\
B \cdot u^2 = B u^2 \\
B \cdot u = B u \\
B \cdot 1 = B
\]
Sum:
- \(u^3: A\)
- \(u^2: A + B\)
- \(u: A + B\)
- const: \(B\)

From \((C u + D)(u^2 + 1)\):

\[
C u \cdot u^2 = C u^3 \\
C u \cdot 1 = C u \\
D \cdot u^2 = D u^2 \\
D \cdot 1 = D
\]
So:
- \(u^3: C\)
- \(u^2: D\)
- \(u: C\)
- const: D

Now, add:
- \(u^3: A + C\)
- \(u^2: A + B + D\)
- \(u: A + B + C\)
- const: \(B + D\)

Wait, when checking the sum for \(u\):
- \(A u\) + \(B u\) + \(C u\) = \(A u\) + \(B u\) (from first factor), \(C u\) (from second), so sum \(A u + B u + C u = (A + B + C)u\).

So the matching is:

\[
2u^3 + 2u^2 + 3u + 2 = (A + C) u^3 + (A + B + D) u^2 + (A + B + C) u + (B + D)
\]

Now, match coefficients:

- \(u^3\): \(A + C = 2\)
- \(u^2\): \(A + B + D = 2\)
- \(u^1\): \(A + B + C = 3\)
- constant: \(B + D = 2\)

So equations:
\[
1.\quad A + C = 2 \\
2.\quad A + B + D = 2 \\
3.\quad A + B + C = 3 \\
4.\quad B + D = 2 \\
\]

Let’s solve:

From (1): \(C = 2 - A\).

From (4): \(D = 2 - B\).

Plug into (2):

(2): \(A + B + D = 2 \Rightarrow A + B + (2 - B) = 2 \implies A + 2 = 2 \implies A = 0\).

Then from (1): \(C = 2 - 0 = 2\).

From (4): \(D = 2 - B\).

From (3): \(A + B + C = 3\):

\(0 + B + 2 = 3 \implies B = 1\).

So, \(B = 1\).

Thus, \(D = 2 - 1 = 1\).

So, the coefficients are:
\[
A = 0,\; B = 1,\; C = 2,\; D = 1
\]

Therefore, the decomposition is:
\[
\frac{2u^3 + 2u^2 + 3u + 2}{(u^2 + 1)(u^2 + u + 1)} = \frac{1}{u^2 + 1} + \frac{2u + 1}{u^2 + u + 1}
\]

So the integral is:
\[
I = \int_0^1 \left[ \frac{1}{u^2 + 1} + \frac{2u + 1}{u^2 + u + 1} \right] du
\]

---

### Step 5: Integrate Each Term

#### First term:

\[
\int_0^1 \frac{1}{u^2 + 1} du = \arctan(u) \Big|_0^1 = \arctan(1) - \arctan(0) = \frac{\pi}{4} - 0 = \frac{\pi}{4}
\]

#### Second term:

\[
\int_0^1 \frac{2u + 1}{u^2 + u + 1} du
\]

Let’s let’s perform substitution.

Let’s denote \( D(u) = u^2 + u + 1 \), then \( D'(u) = 2u + 1 \).

Thus,
\[
\int \frac{2u + 1}{u^2 + u + 1} du = \int \frac{D'(u)}{D(u)} du = \ln| D(u) | + C
\]

So,
\[
\int_0^1 \frac{2u + 1}{u^2 + u + 1} du = \ln(u^2 + u + 1) \Big|_0^1
\]
Evaluate endpoints:

At \(u = 1\):
\[
1^2 + 1 + 1 = 1 + 1 + 1 = 3
\]

At \(u = 0\):
\[
0^2 + 0 + 1 = 1
\]

Thus,
\[
\ln(3) - \ln(1) = \ln(3) - 0 = \ln(3)
\]

---

### Step 6: Final Answer

Add both:

\[
I = \frac{\pi}{4} + \ln(3)
\]

---

### Step 7: Numerical Approximation

Let’s compute:

\[
\frac{\pi}{4} \approx 0.7853981634
\]
\[
\ln(3) \approx 1.0986122887
\]
\[
I \approx 0.7853981634 + 1.0986122887 = 1.8840104521
\]

Rounded to 10 decimal places: **1.8840104521**

---

### Step 8: JSON Output

```json
{"answer": "\\frac{\\pi}{4}+\\ln(3)", "numerical_answer": "1.8840104521"}
```