To solve the definite integral \(\int_0^1 \sqrt[3]{x} \left\lfloor \frac{1}{\sqrt[3]{x}} \right\rfloor \, dx\), we follow these steps:

### Step 1: Substitution
Let \( t = \frac{1}{\sqrt[3]{x}} \). Then:
- \( x = t^{-3} \)
- \( dx = -3t^{-4} \, dt \)
- When \( x = 0 \), \( t \to \infty \)
- When \( x = 1 \), \( t = 1 \)

The integral becomes:
\[
\int_{\infty}^1 t^{-1} \lfloor t \rfloor (-3t^{-4}) \, dt = 3 \int_1^\infty t^{-5} \lfloor t \rfloor \, dt
\]

### Step 2: Break into Sum of Integrals
The floor function \( \lfloor t \rfloor \) is constant on intervals \([n, n+1)\) for integer \( n \geq 1 \). Thus:
\[
3 \int_1^\infty t^{-5} \lfloor t \rfloor \, dt = 3 \sum_{n=1}^\infty n \int_n^{n+1} t^{-5} \, dt
\]

### Step 3: Compute Each Integral
\[
\int_n^{n+1} t^{-5} \, dt = \left[ -\frac{1}{4} t^{-4} \right]_n^{n+1} = \frac{1}{4} \left( n^{-4} - (n+1)^{-4} \right)
\]

Thus, the sum becomes:
\[
3 \sum_{n=1}^\infty n \cdot \frac{1}{4} \left( n^{-4} - (n+1)^{-4} \right) = \frac{3}{4} \sum_{n=1}^\infty \left( n^{-3} - n(n+1)^{-4} \right)
\]

### Step 4: Simplify the Sum
The sum telescopes:
\[
\sum_{n=1}^\infty \left( n^{-3} - n(n+1)^{-4} \right) = \sum_{n=1}^\infty n^{-3} - \sum_{n=1}^\infty n(n+1)^{-4}
\]

The second sum can be rewritten as:
\[
\sum_{n=1}^\infty n(n+1)^{-4} = \sum_{m=2}^\infty (m-1)m^{-4} = \sum_{m=1}^\infty (m-1)m^{-4} = \sum_{m=1}^\infty m^{-3} - \sum_{m=1}^\infty m^{-4}
\]

Thus, the original sum simplifies to:
\[
\sum_{n=1}^\infty n^{-3} - \left( \sum_{n=1}^\infty n^{-3} - \sum_{n=1}^\infty n^{-4} \right) = \sum_{n=1}^\infty n^{-4} = \zeta(4)
\]

### Step 5: Final Calculation
We know that \( \zeta(4) = \frac{\pi^4}{90} \), so:
\[
\frac{3}{4} \cdot \zeta(4) = \frac{3}{4} \cdot \frac{\pi^4}{90} = \frac{\pi^4}{120}
\]

### Numerical Approximation
The numerical value of \( \frac{\pi^4}{120} \) is approximately \( 0.8117424252 \).

### Final Answer
```json
{"answer": "\\frac{\\pi^4}{120}", "numerical_answer": "0.8117424252"}
```