

To solve the definite integral \(\int\limits_0^2 x H_{3}\left(\sqrt{x(2-x)}\right)dx\), we follow these steps:

### Step 1: Recall the Hermite polynomial \(H_3(z)\)
The third Hermite polynomial is \(H_3(z) = 8z^3 - 12z\). Substituting \(z = \sqrt{x(2-x)}\), the integrand becomes:
\[
x \cdot \left[8\left(\sqrt{x(2-x)}\right)^3 - 12\left(\sqrt{x(2-x)}\right)\right]
\]

### Step 2: Simplify the integrand
Let \(t = \sqrt{x(2-x)}\), so \(t^2 = x(2-x)\). The integrand simplifies to:
\[
x \cdot \left[8(x(2-x))^{3/2} - 12(x(2-x))^{1/2}\right]
\]
Expanding, the integral splits into two terms:
\[
8\int_0^2 x \cdot (x(2-x))^{3/2} \, dx - 12\int_0^2 x \cdot (x(2-x))^{1/2} \, dx
\]

### Step 3: Rewrite the integrals using Beta functions
The integrals can be expressed in terms of the Beta function \(B(p, q) = \int_0^1 t^{p-1}(1-t)^{q-1}dt\), related to the Gamma function by \(B(p, q) = \frac{\Gamma(p)\Gamma(q)}{\Gamma(p+q)}\).

For the first integral:
\[
\int_0^2 x^{5/2}(2-x)^{3/2} \, dx
\]
Let \(x = 2t\) (so \(dx = 2dt\)), transforming the integral to:
\[
2^{5/2 + 3/2 + 1} \int_0^1 t^{5/2}(1-t)^{3/2} \, dt = 32 \cdot B\left(\frac{7}{2}, \frac{5}{2}\right)
\]
Using \(\Gamma\left(\frac{7}{2}\right) = \frac{15\sqrt{\pi}}{8}\), \(\Gamma\left(\frac{5}{2}\right) = \frac{3\sqrt{\pi}}{4}\), and \(\Gamma(6) = 120\), we find:
\[
B\left(\frac{7}{2}, \frac{5}{2}\right) = \frac{\Gamma\left(\frac{7}{2}\right)\Gamma\left(\frac{5}{2}\right)}{\Gamma(6)} = \frac{45\pi}{3840} = \frac{3\pi}{256}
\]
Thus, the first integral is \(32 \cdot \frac{3\pi}{256} = \frac{3\pi}{8}\).

For the second integral:
\[
\int_0^2 x^{3/2}(2-x)^{1/2} \, dx
\]
Similarly, \(x = 2t\) transforms it to:
\[
2^{3/2 + 1/2 + 1} \int_0^1 t^{3/2}(1-t)^{1/2} \, dt = 8 \cdot B\left(\frac{5}{2}, \frac{3}{2}\right)
\]
Using \(\Gamma\left(\frac{5}{2}\right) = \frac{3\sqrt{\pi}}{4}\), \(\Gamma\left(\frac{3}{2}\right) = \frac{\sqrt{\pi}}{2}\), and \(\Gamma(4) = 6\), we find:
\[
B\left(\frac{5}{2}, \frac{3}{2}\right) = \frac{\Gamma\left(\frac{5}{2}\right)\Gamma\left(\frac{3}{2}\right)}{\Gamma(4)} = \frac{3\pi}{48} = \frac{\pi}{16}
\]
Thus, the second integral is \(8 \cdot \frac{\pi}{16} = \frac{\pi}{2}\).

### Step 4: Combine the results
The original integral becomes:
\[
8 \cdot \frac{3\pi}{8} - 12 \cdot \frac{\pi}{2} = 3\pi - 6\pi = -3\pi
\]

### Step 5: Numerical approximation
The numerical value of \(-3\pi\) is approximately \(-9.4247779608\) (rounded to 10 decimal places).

{"answer": "$-3\\pi$", "numerical_answer": "-9.4247779608"}