# Evaluating $\int\limits_0^{2.0}x^{1.0-3/2}(2.0-x)^{1.0-1/2}[1-0.5x(2.0-x)]^{-1.0} dx$

First, let's simplify the integrand. We have:
- $x^{1.0-3/2} = x^{-0.5} = \frac{1}{\sqrt{x}}$
- $(2.0-x)^{1.0-1/2} = (2.0-x)^{0.5} = \sqrt{2.0-x}$
- $[1-0.5x(2.0-x)]^{-1.0} = \frac{1}{1-0.5x(2.0-x)}$

So our integral becomes:
$$\int\limits_0^{2.0}\frac{\sqrt{2.0-x}}{\sqrt{x}[1-0.5x(2.0-x)]} dx$$

Let's expand the denominator term:
$$1-0.5x(2.0-x) = 1-0.5(2.0x-x^2) = 1-1.0x+0.5x^2 = 0.5x^2-1.0x+1$$

This can be rewritten as:
$$0.5x^2-1.0x+1 = 0.5(x^2-2x+2) = 0.5[(x-1)^2+1]$$

So our integral becomes:
$$\int\limits_0^{2.0}\frac{\sqrt{2.0-x}}{\sqrt{x} \cdot 0.5[(x-1)^2+1]} dx = 2\int\limits_0^{2.0}\frac{\sqrt{2.0-x}}{\sqrt{x}[(x-1)^2+1]} dx$$

This is a complex integral that can be evaluated using substitution methods. Let's make the substitution $u = \sqrt{\frac{2.0-x}{x}}$.

When $x = 0$, $u = \infty$
When $x = 2.0$, $u = 0$

With this substitution:
- $x = \frac{2.0}{1+u^2}$
- $dx = \frac{-4.0u}{(1+u^2)^2}du$
- $\sqrt{x} = \sqrt{\frac{2.0}{1+u^2}} = \frac{\sqrt{2.0}}{\sqrt{1+u^2}}$
- $\sqrt{2.0-x} = \sqrt{2.0-\frac{2.0}{1+u^2}} = \sqrt{\frac{2.0u^2}{1+u^2}} = \frac{\sqrt{2.0}u}{\sqrt{1+u^2}}$
- $(x-1)^2+1 = \left(\frac{2.0}{1+u^2}-1\right)^2+1 = \left(\frac{2.0-1-u^2}{1+u^2}\right)^2+1 = \left(\frac{1-u^2}{1+u^2}\right)^2+1$

After calculations, we get:
$$(x-1)^2+1 = \frac{(1-u^2)^2+(1+u^2)^2}{(1+u^2)^2} = \frac{2+2u^4}{(1+u^2)^2}$$

Substituting all these into our integral:
$$2\int\limits_{\infty}^{0}\frac{\frac{\sqrt{2.0}u}{\sqrt{1+u^2}}}{\frac{\sqrt{2.0}}{\sqrt{1+u^2}} \cdot \frac{2+2u^4}{(1+u^2)^2}} \cdot \frac{-4.0u}{(1+u^2)^2}du$$

After simplification:
$$2\int\limits_{\infty}^{0}\frac{-4.0u^2}{(2+2u^4)} du = -4\int\limits_{\infty}^{0}\frac{u^2}{2(1+u^4)} du$$

Reversing the limits:
$$4\int\limits_{0}^{\infty}\frac{u^2}{2(1+u^4)} du = 2\int\limits_{0}^{\infty}\frac{u^2}{1+u^4} du$$

Using standard integrals or partial fractions, this evaluates to:
$$2 \cdot \frac{\pi}{2\sqrt{2}} = \frac{\pi}{\sqrt{2}} = \frac{\pi\sqrt{2}}{2}$$

Therefore:
$$\int\limits_0^{2.0}x^{1.0-3/2}(2.0-x)^{1.0-1/2}[1-0.5x(2.0-x)]^{-1.0} dx = \frac{\pi\sqrt{2}}{2}$$

Numerical approximation to 10 decimal places:
$$\frac{\pi\sqrt{2}}{2} \approx 2.2214414690$$

{"answer": "\\frac{\\pi\\sqrt{2}}{2}", "numerical_answer": "2.2214414690"}