We wish to evaluate

  I = ∫₋₄⁴ e^|x| · {x} dx

where {x} is the fractional part of x (defined by {x} = x − ⎣x⎦).

Step 1. Split the integration region into intervals on which the floor function is constant. Notice that the integration limits −4 and 4 are integers. We break the interval into “unit intervals”:
  for x in [n, n+1) with n an integer.
Since −4 ≤ x < 4, we have two groups:
 • For n = −4, −3, −2, −1   (x in [n, n+1) ⊂ [−4, 0))
 • For n = 0, 1, 2, 3      (x in [n, n+1) ⊂ [0, 4))
On each interval, {x} = x − n.

Step 2. Express the integral as a sum.
For each integer n the contribution is
  Iₙ = ∫ₙ^(n+1) e^|x| · (x − n) dx.
Note that the absolute value gives two cases:
 a) For x < 0 (n negative), |x| = −x so e^|x| = e^(−x).
 b) For x ≥ 0 (n nonnegative), |x| = x so e^|x| = e^x.

Thus we write:
  I = Σₙ₌₋₄^(−1) ∫ₙ^(n+1) e^(−x) · (x − n) dx  +  Σₙ₌₀³ ∫ₙ^(n+1) e^x · (x − n) dx.

Step 3. Make a substitution in each unit interval.
Let u = x − n so that x = n + u and du = dx. Then, u runs from 0 to 1.
• For n negative:
  Iₙ = ∫₀¹ e^(−(n+u)) · u du = e^(−n) ∫₀¹ u e^(−u) du.
• For n nonnegative:
  Iₙ = ∫₀¹ e^(n+u) · u du = e^n ∫₀¹ u e^u du.

Step 4. Compute the u-integrals.
Define
  I₁ = ∫₀¹ u e^(−u) du  and  I₂ = ∫₀¹ u e^u du.

To compute I₁:
 You can integrate by parts. Alternatively, note that
 ∫ u e^(−u) du = –e^(−u)(u+1) + C.
Evaluating from 0 to 1 gives:
 I₁ = [–e^(−1)(1+1)] – [–e^(0)(0+1)] = –2e^(−1) + 1 = 1 – (2/e).

For I₂:
 A known antiderivative is
 ∫ u e^u du = e^u(u – 1) + C.
Evaluating from 0 to 1 gives:
 I₂ = [e(1–1)] – [1(0–1)] = 0 + 1 = 1.

Step 5. Write the total sum.
For negative intervals (n = −4, −3, −2, −1), each contributes:
 e^(−n)·I₁ = e^(−n)·(1 – 2/e).
Thus, their sum is
 (1 – 2/e) [e^(4) + e^(3) + e^(2) + e^(1)].
For nonnegative intervals (n = 0, 1, 2, 3), each contributes:
 e^n·I₂ = e^n.
Their sum is
 1 + e + e^2 + e^3.

So,
 I = (1 – 2/e)(e + e^2 + e^3 + e^4) + (1 + e + e^2 + e^3).

Step 6. Simplify the expression.
First expand the product:
 (1 – 2/e)(e + e^2 + e^3 + e^4)
  = (e + e^2 + e^3 + e^4) – (2/e)(e + e^2 + e^3 + e^4)
  = (e + e^2 + e^3 + e^4) – 2(1 + e + e^2 + e^3).
Thus,
 I = [e + e^2 + e^3 + e^4 – 2(1 + e + e^2 + e^3)] + [1 + e + e^2 + e^3].
Combine the terms:
 The sum of the last two groups:
  (e + e^2 + e^3 + e^4) – 2 – 2e – 2e^2 – 2e^3 + 1 + e + e^2 + e^3
 = e^4 + (e + e^2 + e^3 – 2e – 2e^2 – 2e^3 + e + e^2 + e^3) – 2 + 1.
Notice that (e + e^2 + e^3 – 2e – 2e^2 – 2e^3 + e + e^2 + e^3) cancels completely:
 (e – 2e + e) = 0, similarly for e² and e³.
Also −2 + 1 = −1.
Thus, I = e^4 − 1.

Step 7. Provide the numerical approximation.
We have
 e^4 ≈ 54.598150033144236,
so
 I ≈ 54.598150033144236 − 1 = 53.598150033144236.
Rounded to 10 decimal places, I ≈ 53.5981500331.

Final JSON output:
{"answer": "$e^4 - 1$", "numerical_answer": "53.5981500331"}