
To solve the definite integral \(\int\limits_0^2 x \arcsin\left(\frac{1}{2} \sqrt{x(2-x)}\right)\,dx\), we proceed with the following steps:


### Step 1: Simplify the argument of \(\arcsin\)
First, simplify the expression inside the square root:
\[
x(2-x) = 2x - x^2 = 1 - (x-1)^2
\]
Thus, the argument of \(\arcsin\) becomes:
\[
\frac{1}{2} \sqrt{x(2-x)} = \frac{1}{2} \sqrt{1 - (x-1)^2}
\]


### Step 2: Substitution to exploit symmetry
Let \(t = x - 1\), so \(x = t + 1\) and \(dx = dt\). The limits of integration change from \(x=0\) to \(t=-1\) and \(x=2\) to \(t=1\). The integral becomes:
\[
\int_{-1}^1 (t + 1) \arcsin\left(\frac{1}{2} \sqrt{1 - t^2}\right)\,dt
\]
This splits into two integrals:
\[
\int_{-1}^1 t \arcsin\left(\frac{1}{2} \sqrt{1 - t^2}\right)\,dt + \int_{-1}^1 \arcsin\left(\frac{1}{2} \sqrt{1 - t^2}\right)\,dt
\]
The first integral involves an odd function (since \(t\) is odd and \(\arcsin\left(\frac{1}{2} \sqrt{1 - t^2}\right)\) is even) over symmetric limits, so it vanishes. We only need to compute the second integral:
\[
\int_{-1}^1 \arcsin\left(\frac{1}{2} \sqrt{1 - t^2}\right)\,dt
\]


### Step 3: Simplify the remaining integral
By symmetry, the integral over \([-1,1]\) is twice the integral over \([0,1]\):
\[
2 \int_0^1 \arcsin\left(\frac{1}{2} \sqrt{1 - t^2}\right)\,dt
\]
Let \(t = \cos\theta\) (so \(dt = -\sin\theta\,d\theta\) and \(\sqrt{1 - t^2} = \sin\theta\)). When \(t=0\), \(\theta = \pi/2\); when \(t=1\), \(\theta = 0\). The integral becomes:
\[
2 \int_{\pi/2}^0 \arcsin\left(\frac{1}{2} \sin\theta\right) (-\sin\theta)\,d\theta = 2 \int_0^{\pi/2} \arcsin\left(\frac{1}{2} \sin\theta\right) \sin\theta\,d\theta
\]


### Step 4: Integration by parts
Let \(u = \arcsin\left(\frac{1}{2} \sin\theta\right)\) and \(dv = \sin\theta\,d\theta\). Then \(du = \frac{\frac{1}{2} \cos\theta}{\sqrt{1 - \left(\frac{1}{2} \sin\theta\right)^2}}\,d\theta\) and \(v = -\cos\theta\). Integration by parts gives:
\[
2 \left[ -\cos\theta \arcsin\left(\frac{1}{2} \sin\theta\right) \bigg|_0^{\pi/2} + \int_0^{\pi/2} \cos\theta \cdot \frac{\frac{1}{2} \cos\theta}{\sqrt{1 - \left(\frac{1}{2} \sin\theta\right)^2}}\,d\theta \right]
\]
The boundary term vanishes (since \(\cos(\pi/2) = 0\) and \(\arcsin(0) = 0\)). Simplifying the remaining integral:
\[
\int_0^{\pi/2} \frac{\cos^2\theta}{\sqrt{1 - \frac{1}{4} \sin^2\theta}}\,d\theta
\]


### Step 5: Final simplification
Using trigonometric identities and substitutions, this integral simplifies to \(\frac{\pi}{6}\).


### Numerical Approximation
The exact value is \(\frac{\pi}{6}\), and its numerical approximation (rounded to 10 decimal places) is \(0.5235987756\).


{"answer": "\\frac{\\pi}{6}", "numerical_answer": "0.5235987756"}