To solve the definite integral 

\[
\int_0^{\pi/4} \frac{\tan(x) + 2\sec^2(x) + 2\tan(x)\sec^2(x)}{\tan(x) + \sec^2(x)} \, dx,
\]

we follow these steps:

### Step 1: Simplify the Integrand
First, let's simplify the integrand. Notice that the denominator is \(\tan(x) + \sec^2(x)\). Recall that \(\sec^2(x) = 1 + \tan^2(x)\), so the denominator can be rewritten as:

\[
\tan(x) + \sec^2(x) = \tan(x) + 1 + \tan^2(x) = \tan^2(x) + \tan(x) + 1.
\]

Letâ€™s set \( u = \tan(x) \). Then, \( du = \sec^2(x) \, dx \). 

The numerator is:

\[
\tan(x) + 2\sec^2(x) + 2\tan(x)\sec^2(x) = u + 2(1 + u^2) + 2u(1 + u^2) = u + 2 + 2u^2 + 2u + 2u^3 = 2u^3 + 2u^2 + 3u + 2.
\]

The denominator is:

\[
\tan^2(x) + \tan(x) + 1 = u^2 + u + 1.
\]

Thus, the integrand becomes:

\[
\frac{2u^3 + 2u^2 + 3u + 2}{u^2 + u + 1}.
\]

### Step 2: Perform Polynomial Division
We perform polynomial division on the numerator by the denominator:

\[
2u^3 + 2u^2 + 3u + 2 = (2u)(u^2 + u + 1) + (u + 2).
\]

So, the integrand simplifies to:

\[
2u + \frac{u + 2}{u^2 + u + 1}.
\]

### Step 3: Integrate Term by Term
Now, the integral becomes:

\[
\int \left(2u + \frac{u + 2}{u^2 + u + 1}\right) du = \int 2u \, du + \int \frac{u + 2}{u^2 + u + 1} \, du.
\]

The first integral is straightforward:

\[
\int 2u \, du = u^2 + C.
\]

For the second integral, we complete the square in the denominator:

\[
u^2 + u + 1 = \left(u + \frac{1}{2}\right)^2 + \frac{3}{4}.
\]

Let \( v = u + \frac{1}{2} \), so \( dv = du \), and \( u = v - \frac{1}{2} \). The numerator \( u + 2 \) becomes:

\[
u + 2 = v - \frac{1}{2} + 2 = v + \frac{3}{2}.
\]

Thus, the second integral becomes:

\[
\int \frac{v + \frac{3}{2}}{v^2 + \frac{3}{4}} \, dv = \int \frac{v}{v^2 + \frac{3}{4}} \, dv + \frac{3}{2} \int \frac{1}{v^2 + \frac{3}{4}} \, dv.
\]

The first part is:

\[
\int \frac{v}{v^2 + \frac{3}{4}} \, dv = \frac{1}{2} \ln\left(v^2 + \frac{3}{4}\right) + C.
\]

The second part is:

\[
\frac{3}{2} \int \frac{1}{v^2 + \frac{3}{4}} \, dv = \frac{3}{2} \cdot \frac{2}{\sqrt{3}} \arctan\left(\frac{2v}{\sqrt{3}}\right) + C = \sqrt{3} \arctan\left(\frac{2v}{\sqrt{3}}\right) + C.
\]

### Step 4: Substitute Back and Evaluate
Substituting back \( v = u + \frac{1}{2} \), the second integral becomes:

\[
\frac{1}{2} \ln\left(\left(u + \frac{1}{2}\right)^2 + \frac{3}{4}\right) + \sqrt{3} \arctan\left(\frac{2u + 1}{\sqrt{3}}\right) + C.
\]

Now, combine with the first integral:

\[
u^2 + \frac{1}{2} \ln(u^2 + u + 1) + \sqrt{3} \arctan\left(\frac{2u + 1}{\sqrt{3}}\right) + C.
\]

Recall that \( u = \tan(x) \). The limits of integration are \( x = 0 \) to \( x = \pi/4 \), which correspond to \( u = 0 \) to \( u = 1 \).

### Step 5: Evaluate the Definite Integral
Evaluate the expression from \( u = 0 \) to \( u = 1 \):

At \( u = 1 \):

\[
1^2 + \frac{1}{2} \ln(1^2 + 1 + 1) + \sqrt{3} \arctan\left(\frac{2 \cdot 1 + 1}{\sqrt{3}}\right) = 1 + \frac{1}{2} \ln(3) + \sqrt{3} \arctan\left(\sqrt{3}\right) = 1 + \frac{1}{2} \ln(3) + \sqrt{3} \cdot \frac{\pi}{3}.
\]

At \( u = 0 \):

\[
0^2 + \frac{1}{2} \ln(0^2 + 0 + 1) + \sqrt{3} \arctan\left(\frac{2 \cdot 0 + 1}{\sqrt{3}}\right) = 0 + \frac{1}{2} \ln(1) + \sqrt{3} \arctan\left(\frac{1}{\sqrt{3}}\right) = 0 + 0 + \sqrt{3} \cdot \frac{\pi}{6}.
\]

Subtracting the lower limit from the upper limit:

\[
\left(1 + \frac{1}{2} \ln(3) + \frac{\sqrt{3} \pi}{3}\right) - \left(\frac{\sqrt{3} \pi}{6}\right) = 1 + \frac{1}{2} \ln(3) + \frac{\sqrt{3} \pi}{6}.
\]

### Step 6: Numerical Approximation
The exact answer is:

\[
1 + \frac{1}{2} \ln(3) + \frac{\sqrt{3} \pi}{6}.
\]

Numerically approximating this:

\[
1 + \frac{1}{2} \ln(3) \approx 1 + 0.5493061443 \approx 1.5493061443,
\]
\[
\frac{\sqrt{3} \pi}{6} \approx \frac{1.7320508075 \cdot 3.1415926535}{6} \approx 0.9068996821,
\]
\[
1.5493061443 + 0.9068996821 \approx 2.4562058264.
\]

Rounding to 10 decimal places:

\[
2.4562058264.
\]

### Final Answer
```json
{"answer": "1 + \\frac{1}{2} \\ln(3) + \\frac{\\sqrt{3} \\pi}{6}", "numerical_answer": "2.4562058264"}
```