We will show that a “lucky” choice of rewriting the integrand produces an answer in closed‐form. (A standard method such as “integration by parts” might lead to a very messy antiderivative.) Notice that
  sin(101x) = sin(100x + x) = sin(100x) cos x + cos(100x) sin x.
Thus
  sin(101x)·sin^(99)x = sin(100x)·(cos x·sin^(99)x) + cos(100x)·(sin^(100)x).

Now observe that if we differentiate
  F(x) = sin(100x)·sin^(100)x,
we obtain by the product rule
  F′(x) = 100 cos(100x)·sin^(100)x + sin(100x)·100 sin^(99)x·cos x
     = 100 sin^(99)x [cos(100x)·sin x + sin(100x)·cos x]
     = 100 sin^(99)x·sin(101x).
That is,
  F′(x) = 100 sin(101x) sin^(99)x.
It follows that an antiderivative for sin(101x)·sin^(99)x is
  ∫ sin(101x) sin^(99)x dx = (1/100) sin(100x)·sin^(100)x + C.

For the numerical approximation we “evaluate” the antiderivative at a particular value. (Since no limits were specified the antiderivative is determined only up to an arbitrary constant; here we choose x = 1 for a representative numeric value.) That is, define
  A = (1/100) sin(100)·[sin(1)]^(100).

A short computation gives:
 • 100 (in radians) reduced modulo 2π gives a remainder approximately 5.75222039 so that
  sin(100) ≈ –0.505
 • Also, sin(1) ≈ 0.8414709848 and then [0.8414709848]^(100) = exp(100·ln(0.8414709848)) ≈ exp(–17.2) ≈ 3.363×10^(–8).
Thus,
  A ≈ (1/100)·(–0.505)·(3.363×10^(–8)) ≈ –1.70×10^(–10).

We now output the final answer in the required JSON format.

{"answer": "\\frac{\\sin(100x)\\,\\sin^{100}(x)}{100} + C", "numerical_answer": "-1.7000000000e-10"}