
To solve the definite integral \(\int\limits_{0}^{1}x^{-1/2}\left[1-\sqrt{x(1-x)}\right]^{-2}dx\), we proceed with the following steps:

### Step 1: Substitution \(t = \sqrt{x}\)
Let \(t = \sqrt{x}\), so \(x = t^2\) and \(dx = 2t \, dt\). The limits of integration become \(t = 0\) (when \(x = 0\)) and \(t = 1\) (when \(x = 1\)). Substituting these into the integral:
\[
\int_{0}^{1} x^{-1/2} \left[1 - \sqrt{x(1-x)}\right]^{-2} dx = \int_{0}^{1} (t^2)^{-1/2} \left[1 - \sqrt{t^2(1 - t^2)}\right]^{-2} \cdot 2t \, dt
\]
Simplifying \(x^{-1/2} = t^{-1}\) and \(\sqrt{x(1-x)} = t\sqrt{1 - t^2}\), the integral reduces to:
\[
2 \int_{0}^{1} \left[1 - t\sqrt{1 - t^2}\right]^{-2} dt
\]

### Step 2: Trigonometric Substitution \(t = \sin\theta\)
Let \(t = \sin\theta\), so \(dt = \cos\theta \, d\theta\) and \(\sqrt{1 - t^2} = \cos\theta\). The limits of integration become \(\theta = 0\) (when \(t = 0\)) and \(\theta = \frac{\pi}{2}\) (when \(t = 1\)). Substituting these:
\[
2 \int_{0}^{\pi/2} \left[1 - \sin\theta \cos\theta\right]^{-2} \cos\theta \, d\theta
\]

### Step 3: Symmetry and Substitution \(t = \sin\theta - \cos\theta\)
Consider the integral with \(\phi = \frac{\pi}{2} - \theta\), which transforms the integral into:
\[
2 \int_{0}^{\pi/2} \left[1 - \sin\phi \cos\phi\right]^{-2} \sin\phi \, d\phi
\]
Adding the two expressions for the integral and simplifying, we find:
\[
I = \int_{0}^{\pi/2} \frac{\cos\theta + \sin\theta}{\left[1 - \sin\theta \cos\theta\right]^2} d\theta
\]
Let \(u = \sin\theta - \cos\theta\), so \(du = (\cos\theta + \sin\theta) d\theta\). The term \(1 - \sin\theta \cos\theta\) simplifies to \(\frac{1 + u^2}{2}\), and the limits of \(u\) are \(-1\) to \(1\). The integral becomes:
\[
I = \int_{-1}^{1} \frac{4}{(1 + u^2)^2} du
\]

### Step 4: Evaluating the Integral
The integral \(\int \frac{1}{(1 + u^2)^2} du\) has the antiderivative \(\frac{u}{2(1 + u^2)} + \frac{1}{2} \arctan u\). Evaluating from \(-1\) to \(1\):
\[
\int_{-1}^{1} \frac{4}{(1 + u^2)^2} du = 4 \left[ \frac{u}{2(1 + u^2)} + \frac{1}{2} \arctan u \right]_{-1}^{1} = 2 + \pi
\]

### Numerical Approximation
The exact value is \(2 + \pi\). Numerically, \(\pi \approx 3.141592653589793\), so \(2 + \pi \approx 5.1415926536\).

### Final Answer
{"answer": "2 + \pi", "numerical_answer": "5.1415926536"}