We wish to evaluate

  I = ∫₀^(π/2) x·ln(sin x) dx.

A very efficient method is to use the Fourier series expansion for ln(sin x). In particular, for 0 < x < π we have

  ln(sin x) = -ln 2 − ∑ₘ₌₁^(∞) (cos(2m x) / m).

Thus, we write

  I = ∫₀^(π/2) x ( -ln 2 − ∑ₘ₌₁^(∞) (cos(2m x)/m) ) dx
    = -ln2 ∫₀^(π/2) x dx − ∑ₘ₌₁^(∞) (1/m) ∫₀^(π/2) x cos(2m x) dx.

Step 1. Evaluate the first term:
  ∫₀^(π/2) x dx = [x²/2]₀^(π/2) = (π/2)²/2 = π²/8.
Thus, the first term equals
  -ln2 · (π²/8) = - (π² ln2)/8.

Step 2. Evaluate the second term.
We need to compute Jₘ = ∫₀^(π/2) x cos(2m x) dx for m = 1, 2, 3, ….
We use integration by parts:
  Let u = x  ⇒ du = dx,
  dv = cos(2m x) dx  ⇒ v = sin(2m x)/(2m).
Thus,
  Jₘ = [x sin(2m x)/(2m)]₀^(π/2) - ∫₀^(π/2) (sin(2m x)/(2m)) dx.
Now, compute the boundary term:
  At x = π/2: sin(2m (π/2)) = sin(mπ) = 0;
  At x = 0: x = 0.
So, the first term vanishes.
Next, compute the second integral:
  ∫₀^(π/2) sin(2m x) dx = [ -cos(2m x)/(2m) ]₀^(π/2)
    = - [cos(mπ) - cos 0] / (2m)
    = - [(-1)ᵐ - 1] / (2m).
Thus,
  Jₘ = - (1/(2m)) · { - [(-1)ᵐ - 1] / (2m) } = ([(-1)ᵐ - 1])/(4m²).

Therefore, the contribution from the sum becomes
  ∑ₘ₌₁^(∞) (1/m) Jₘ = ∑ₘ₌₁^(∞) (( (-1)ᵐ - 1)/(4m³) ).
Notice that (-1)ᵐ - 1 equals 0 when m is even and equals -2 when m is odd. Hence, the sum reduces to
  ∑ₘ₌₁^(∞) (( (-1)ᵐ - 1)/(4m³) ) = (1/4) ∑₍ₘ odd₎ ( -2/(m³) ) = - (1/2) ∑₍ₘ odd₎ 1/(m³).
Recall that the sum over the reciprocals of the cubes of the odd positive integers is given by
  ∑₍ₘ odd₎ 1/(m³) = (1 - 1/2³) ζ(3) = (7/8) ζ(3),
where ζ(3) is Apéry’s constant. Thus, the entire sum is
  - (1/2) · (7/8) ζ(3) = - (7 ζ(3))/(16).

Returning to I, note the minus sign coming from our original formula, so that the second term in I becomes
  - [ - (7 ζ(3))/(16) ] = (7 ζ(3))/(16).

Step 3. Combining the two parts, we find
  I = -(π² ln2)/8 + (7 ζ(3))/(16).

Step 4. Numerical approximation.
Using
  π² ≈ 9.869604401089358,
  ln2 ≈ 0.6931471805599453,
  ζ(3) ≈ 1.2020569031595942,
we compute:
  First term: (π² ln2)/8 ≈ (9.869604401089358 × 0.6931471805599453)/8 ≈ 6.837204/8 ≈ 0.8546505.
Thus, - (π² ln2)/8 ≈ -0.8546505.
  Second term: (7 ζ(3))/16 ≈ (7 × 1.2020569031595942)/16 ≈ 8.414398322/16 ≈ 0.5258999.
Thus,
  I ≈ -0.8546505 + 0.5258999 = -0.3287506.

Finally, the answer in the required JSON format is:

{"answer": "$-\\frac{\\pi^2\\ln2}{8}+\\frac{7\\zeta(3)}{16}$", "numerical_answer": "-0.3287506"}