

To solve the definite integral \(\int\limits_0^2 x^{1/2}(2-x)^{-1/2}\cosh\left(\sqrt{x(2-x)}\right)dx\), we proceed with the following steps:

### Step 1: Simplify the Argument of the Hyperbolic Cosine
First, note that \(x(2 - x) = 2x - x^2 = 1 - (x - 1)^2\). Thus, \(\sqrt{x(2 - x)} = \sqrt{1 - (x - 1)^2}\). We use the substitution \(t = x - 1\), so \(x = t + 1\) and \(dx = dt\). The limits of integration change from \(x = 0\) to \(t = -1\) and \(x = 2\) to \(t = 1\). The integral becomes:
\[
\int_{-1}^1 \sqrt{\frac{t + 1}{1 - t}} \cosh\left(\sqrt{1 - t^2}\right) dt
\]

### Step 2: Trigonometric Substitution
Next, let \(t = \cos\theta\), so \(dt = -\sin\theta d\theta\). When \(t = -1\), \(\theta = \pi\); when \(t = 1\), \(\theta = 0\). Reversing the limits, we rewrite the integral as:
\[
\int_0^\pi \sqrt{\frac{1 + \cos\theta}{1 - \cos\theta}} \cosh(\sin\theta) \sin\theta d\theta
\]
Using the identity \(\frac{1 + \cos\theta}{1 - \cos\theta} = \cot^2\left(\frac{\theta}{2}\right)\), we simplify \(\sqrt{\frac{1 + \cos\theta}{1 - \cos\theta}} = \cot\left(\frac{\theta}{2}\right)\). The integrand becomes:
\[
\cot\left(\frac{\theta}{2}\right) \cosh(\sin\theta) \sin\theta
\]
Since \(\cot\left(\frac{\theta}{2}\right) \sin\theta = 2\cos^2\left(\frac{\theta}{2}\right) = 1 + \cos\theta\), the integral reduces to:
\[
\int_0^\pi (1 + \cos\theta) \cosh(\sin\theta) d\theta
\]

### Step 3: Split the Integral
Split the integral into two parts:
\[
\int_0^\pi \cosh(\sin\theta) d\theta + \int_0^\pi \cos\theta \cosh(\sin\theta) d\theta
\]
For the second integral, let \(u = \sin\theta\), so \(du = \cos\theta d\theta\). The limits become \(u = 0\) to \(u = 0\), making the second integral zero. Thus, we only need to evaluate the first integral:
\[
\int_0^\pi \cosh(\sin\theta) d\theta
\]

### Step 4: Evaluate the Remaining Integral
Using the identity \(\cosh(z) = \frac{e^z + e^{-z}}{2}\), we rewrite the integral as:
\[
\frac{1}{2} \int_0^\pi \left(e^{\sin\theta} + e^{-\sin\theta}\right) d\theta
\]
Both integrals \(\int_0^\pi e^{\sin\theta} d\theta\) and \(\int_0^\pi e^{-\sin\theta} d\theta\) are equal to \(\pi I_0(1)\), where \(I_0\) is the modified Bessel function of the first kind of order 0. Thus:
\[
\int_0^\pi \cosh(\sin\theta) d\theta = \pi I_0(1)
\]

### Final Result
The original integral simplifies to \(\pi I_0(1)\).

### Numerical Approximation
The modified Bessel function \(I_0(1) \approx 1.2660658777520081\). Multiplying by \(\pi\) gives:
\[
\pi I_0(1) \approx 3.9774629220
\]

{"answer": "\(\pi I_0(1)\)", "numerical_answer": "3.9774629220"}