Let \( I = \int_{0}^{1} \arcsin(x) \arccos(x) \, dx \).

---

## Step 1: Simplify the Integral

Recall that \(\arcsin(x) + \arccos(x) = \frac{\pi}{2}\) for \(x \in [0,1]\).

So, \(\arccos(x) = \frac{\pi}{2} - \arcsin(x)\), and thus:

\[
I = \int_{0}^{1} \arcsin(x) \arccos(x) dx = \int_{0}^{1} \arcsin(x) \left(\frac{\pi}{2} - \arcsin(x)\right) dx
\]

\[
= \frac{\pi}{2} \int_{0}^{1} \arcsin(x) dx - \int_{0}^{1} \arcsin^2(x) dx
\]

Let’s call:

\[
A = \int_{0}^{1} \arcsin(x) dx
\]
\[
B = \int_{0}^{1} \arcsin^2(x) dx
\]

So,
\[
I = \frac{\pi}{2}A - B
\]

---

## Step 2: Evaluate \(A = \int_{0}^{1} \arcsin(x) dx\)

Let’s use integration by parts:

Let \(u = \arcsin(x)\), \(dv = dx\), then \(du = \frac{1}{\sqrt{1-x^2}} dx\), and \(v = x\):

\[
A = x \arcsin(x) \Big|_0^1 - \int_0^1 x \cdot \frac{1}{\sqrt{1-x^2}} dx
\]

\[
= [1 \cdot \arcsin(1) - 0 \cdot \arcsin(0)] - \int_0^1 \frac{x}{\sqrt{1-x^2}} dx
\]
\[
= \frac{\pi}{2} - \int_0^1 \frac{x}{\sqrt{1-x^2}} dx
\]

Let’s solve \(\int_0^1 \frac{x}{\sqrt{1-x^2}} dx\):

Let \(u = 1 - x^2\), \(du = -2x dx\), so \(x dx = -\frac{1}{2} du\):

When \(x=0\), \(u=1\); when \(x=1\), \(u=0\):

\[
\int_0^1 \frac{x}{\sqrt{1-x^2}} dx = \int_{u=1}^{u=0} \frac{1}{\sqrt{u}} \cdot \left(-\frac{1}{2} du\right)
= \frac{1}{2} \int_{u=0}^1 u^{-1/2} du
= \frac{1}{2} \cdot \left[2 u^{1/2}\right]_{0}^{1}
= [u^{1/2}]_{0}^{1} = 1-0 = 1
\]

So,
\[
A = \frac{\pi}{2} - 1
\]

---

## Step 3: Evaluate \(B = \int_0^1 \arcsin^2(x) dx\)

We use the reduction formula:
\[
\int \arcsin^n(x) dx
\]
But let’s directly compute:

Let’s use integration by parts: set
- \(u = \arcsin^2(x)\), \(dv = dx\)
- \(du = 2\arcsin(x) \cdot \frac{1}{\sqrt{1-x^2}} dx\), \(v = x\)

So,
\[
B = \int_{0}^{1} \arcsin^2(x) dx = x \arcsin^2(x) \Big|_0^1 - \int_0^1 x \cdot 2\arcsin(x) \cdot \frac{1}{\sqrt{1-x^2}} dx
\]

\[
= [1 \cdot \arcsin^2(1) - 0 \cdot \arcsin^2(0)] - 2 \int_0^1 x \frac{\arcsin(x)}{\sqrt{1-x^2}} dx
\]

Since \(\arcsin(1) = \frac{\pi}{2}\), \(\arcsin(0) = 0\):

\[
= \left(\frac{\pi}{2}\right)^2 - 2 J
\]
where
\[
J = \int_0^1 x \frac{\arcsin(x)}{\sqrt{1-x^2}} dx
\]

Let’s compute \(J\):

Let’s use substitution: \(x = \sin\theta\), \(dx = \cos\theta d\theta\), as \(x\) goes from 0 to 1, \(\theta\) goes from \(0\) to \(\frac{\pi}{2}\):

- \(x = \sin\theta\)
- \(\arcsin(x) = \theta\)
- \(\sqrt{1-x^2} = \sqrt{1-\sin^2\theta} = \cos\theta\)
- \(dx = \cos\theta d\theta\)

Therefore,
\[
J = \int_{x=0}^{x=1} x \frac{\arcsin(x)}{\sqrt{1-x^2}} dx = \int_{\theta=0}^{\theta=\frac{\pi}{2}} \sin\theta \cdot \frac{\theta}{\cos\theta} \cdot \cos\theta d\theta = \int_{0}^{\frac{\pi}{2}} \theta \sin\theta d\theta
\]

Now, compute \(\int_{0}^{\frac{\pi}{2}} \theta \sin\theta d\theta\) by parts:

Let \(u = \theta\), \(dv = \sin\theta d\theta\), so \(du = d\theta\), \(v = -\cos\theta\):

\[
\int \theta \sin\theta d\theta = -\theta \cos\theta + \int \cos\theta d\theta = -\theta \cos\theta + \sin\theta + C
\]

So,

\[
\int_{0}^{\frac{\pi}{2}} \theta \sin\theta d\theta = \left[ -\theta \cos\theta + \sin\theta \right]_{0}^{\frac{\pi}{2}}
\]

At \(\theta = \frac{\pi}{2}\), \(\cos\theta = 0\), \(\sin\theta = 1\)
At \(\theta = 0\), \(\cos\theta = 1\), \(\sin\theta = 0\)

Therefore:

\[
= \left(0 + 1\right) - \left(-0 + 0\right) = 1 - 0 = 1
\]

So, \(J = 1\), and thus

\[
B = \left(\frac{\pi}{2}\right)^2 - 2 \times 1 = \frac{\pi^2}{4} - 2
\]

---

## Step 4: Write Final Expression for \(I\)

Recall:
\[
I = \frac{\pi}{2}A - B = \frac{\pi}{2}\left(\frac{\pi}{2} - 1\right) - \left(\frac{\pi^2}{4} - 2\right)
\]
Expanding:
\[
= \frac{\pi^2}{4} - \frac{\pi}{2} - \frac{\pi^2}{4} + 2
\]
\[
= -\frac{\pi}{2} + 2
\]

---

## Step 5: Numerical Approximation

\[
I = 2 - \frac{\pi}{2} \approx 2 - 1.5707963268 = 0.4292036732
\]

---

## Step 6: JSON Format

```json
{"answer": "2 - \\frac{\\pi}{2}", "numerical_answer": "0.4292036732"}
```