<think>
Okay, so I need to compute the definite integral from 0 to 2.0 of cos(1.0 times the square root of x times (2.0 minus x)) dx. Let me start by writing down the integral properly. The integrand is cos(√(x(2 - x))), and the limits are from 0 to 2. Hmm, maybe there's a substitution that can simplify this expression inside the cosine.

First, let me look at the expression under the square root: x(2 - x). That looks like a quadratic expression. If I complete the square here, maybe I can find a substitution. Let's see, x(2 - x) = -x² + 2x. Completing the square: - (x² - 2x) = -[(x - 1)^2 - 1] = - (x - 1)^2 + 1. So, x(2 - x) = 1 - (x - 1)^2. That's a standard form, which might suggest a trigonometric substitution.

So, the integral becomes ∫ from 0 to 2 cos(√(1 - (x - 1)^2)) dx. Let me make a substitution to simplify the square root. Let’s set u = x - 1. Then, du = dx, and when x = 0, u = -1, and when x = 2, u = 1. So the integral becomes ∫ from u = -1 to u = 1 of cos(√(1 - u²)) du. Wait, but the integrand is symmetric around u = 0 because cos is an even function. So, we can write this as 2 times the integral from 0 to 1 of cos(√(1 - u²)) du. Wait, no, the integrand is cos(√(1 - u²)), which is even because replacing u with -u gives the same function. So, the integral from -1 to 1 is twice the integral from 0 to 1. So, the original integral is 2 * ∫ from 0 to 1 cos(√(1 - u²)) du.

Hmm, but maybe another substitution here. Let me consider t = √(1 - u²). Then, t = √(1 - u²) implies t² = 1 - u², so u² = 1 - t². Differentiating both sides, 2u du = -2t dt, so u du = -t dt. But I need to express du in terms of dt. Wait, solving for du: du = (-t dt)/u. But u = sqrt(1 - t²), so du = (-t dt)/sqrt(1 - t²). Hmm, but this might complicate things. Let me check the limits. When u = 0, t = 1. When u = 1, t = 0. So, the integral becomes ∫ from t=1 to t=0 of cos(t) * (-t dt)/sqrt(1 - t²). Flipping the limits, that's ∫ from 0 to 1 cos(t) * (t dt)/sqrt(1 - t²) = ∫ from 0 to 1 [t cos(t) / sqrt(1 - t²)] dt. Hmm, not sure if that's better. Maybe another substitution.

Alternatively, maybe use polar coordinates or recognize the integral as a Bessel function. Wait, the integral ∫ cos(a sqrt(1 - u²)) du from 0 to 1. Let me check if this is a known integral. Alternatively, maybe use substitution θ = arcsin(u), but let's see. Let me set u = sinθ. Then, when u = 0, θ = 0; when u = 1, θ = π/2. Then, du = cosθ dθ. Then, sqrt(1 - u²) = sqrt(1 - sin²θ) = cosθ. So, the integral becomes ∫ from 0 to π/2 cos(cosθ) * cosθ dθ. Wait, that's ∫0^{π/2} cos(cosθ) cosθ dθ. Hmm, that seems more complicated. Maybe not helpful.

Alternatively, perhaps expand the cosine into its Taylor series and integrate term by term. Let's try that. The integrand is cos(√(1 - u²)). The Taylor series for cos(z) is Σ_{n=0}^∞ (-1)^n z^{2n}/(2n)! So, substituting z = √(1 - u²), we get cos(√(1 - u²)) = Σ_{n=0}^∞ (-1)^n (1 - u²)^n / (2n)! Then, integrating term by term from 0 to 1, the integral becomes Σ_{n=0}^∞ (-1)^n / (2n)! ∫0^1 (1 - u²)^n du. Then, the integral of (1 - u²)^n du from 0 to 1 is known as the Beta function. Specifically, ∫0^1 (1 - u²)^n} du = (sqrt(π)/2) Γ(n + 1)/Γ(n + 3/2). Alternatively, using substitution u = sinθ, then du = cosθ dθ, and the integral becomes ∫0^{π/2} cos^{2n + 1}θ dθ. Which is (sqrt(π)/2) Γ(n + 1)/Γ(n + 3/2). But maybe there's a better way to express this. Alternatively, for integer n, this integral is ( (2n)!! ) / ( (2n + 1)!! ) ). But I need to check.

Wait, the integral ∫0^1 (1 - u²)^n du can be expressed using the Beta function. Let me recall that ∫0^1 u^{k} (1 - u²)^n du can be transformed by substitution t = u², so dt = 2u du, but maybe not necessary here. Alternatively, using substitution t = u², but perhaps more straightforward: ∫0^1 (1 - u²)^n du = 1/2 B(n + 1, 1/2) where B is the Beta function. Since B(a, b) = 2 ∫0^{π/2} (sinθ)^{2a -1} (cosθ)^{2b -1} dθ. Wait, but in our case, the substitution u = sinθ would lead to ∫0^{π/2} cos^{2n + 1}θ dθ. Which is equal to (sqrt(π)/2) Γ(n + 1)/Γ(n + 3/2). So, using the Beta function relation, B(a, b) = Γ(a)Γ(b)/Γ(a + b). So, ∫0^1 (1 - u²)^n du = (1/2) B(n + 1, 1/2) = (1/2) Γ(n + 1)Γ(1/2)/Γ(n + 3/2). Since Γ(1/2) = sqrt(π), this becomes (sqrt(π)/2) Γ(n + 1)/Γ(n + 3/2). 

But Γ(n + 1) = n! and Γ(n + 3/2) can be expressed using the double factorial. Wait, Γ(n + 3/2) = (2n + 1)!! / 2^{n + 1}} sqrt(π). Wait, let me check. For example, Γ(1/2) = sqrt(π), Γ(3/2) = (1/2) sqrt(π), Γ(5/2) = (3/4) sqrt(π), etc. So, in general, Γ(n + 3/2) = (2n + 1)!! / 2^{n + 1}} sqrt(π). Therefore, Γ(n + 1) = n! So, substituting back into the integral:

∫0^1 (1 - u²)^n du = (sqrt(π)/2) * n! / [ (2n + 1)!! / 2^{n + 1} sqrt(π) ) ] = (sqrt(π)/2) * n! * 2^{n + 1} sqrt(π) / (2n + 1)!! ) = (sqrt(π) * 2^{n} * sqrt(π) * n! ) / (2n + 1)!! ) = (π * 2^{n} * n! ) / (2n + 1)!! )

But 2^{n} * n! = (2n)!!, since 2n!! = 2n * 2(n-1) * ... * 2. So, 2^{n} * n! = 2n!!. Wait, no. Wait, n! = 1*2*3*...*n, and 2n!! = 2*4*6*...*2n = 2^n * n!. So, 2n!! = 2^n n!.

Therefore, the integral becomes (π * 2^{n} n! ) / (2n + 1)!! ) = π (2n)! / (2n + 1)!! ) * 2^{n} n! / (2n + 1)!! )? Wait, maybe I made a mistake here. Let me re-express.

Wait, Γ(n + 3/2) = (2n + 1)!! / 2^{n + 1}} sqrt(π). So, substituting back:

∫0^1 (1 - u²)^n du = (sqrt(π)/2) * n! / [ (2n + 1)!! / 2^{n + 1} sqrt(π) ) ] = (sqrt(π)/2) * n! * 2^{n + 1} sqrt(π) / (2n + 1)!! )

Simplify numerator and denominator:

sqrt(π) * 2^{n + 1} sqrt(π) * n! / (2 * (2n + 1)!! )) = (π * 2^{n} * n! ) / ( (2n + 1)!! ) )

Yes, because 2^{n + 1} / 2 = 2^{n}.

So, the integral ∫0^1 (1 - u²)^n du = π (2^{n} n! ) / (2n + 1)!! )

Therefore, going back to the original series expansion:

The integral from 0 to 1 of cos(√(1 - u²)) du = Σ_{n=0}^∞ [ (-1)^n / (2n)! ) * π (2^{n} n! ) / (2n + 1)!! ) ]

Hmm, this seems complicated. Let me see if this series can be simplified. Let's write out the terms:

Each term is (-1)^n * π * 2^{n} n! / [ (2n)! (2n + 1)!! ) ]

But note that (2n)! = (2n)!! (2n - 1)!! ). Because (2n)! = 2n * (2n - 1) * 2(n - 1) * (2n - 3) * ... * 2 * 1 = (2n)!! (2n - 1)!! )

Therefore, (2n)! = (2n)!! (2n - 1)!! )

But 2^{n} n! = (2n)!!, since 2n!! = 2*2(n-1)*...*2*1 = 2^n n!.

So, substituting back into the term:

(-1)^n * π * (2n)!! / [ (2n)!! (2n - 1)!! ) (2n + 1)!! ) ] = (-1)^n * π / [ (2n - 1)!! (2n + 1)!! ) ]

But (2n - 1)!! (2n + 1)!! ) = (2n + 1)!! * (2n - 1)!! = (2n + 1)(2n - 1)!!^2. Hmm, not sure. Alternatively, note that (2n + 1)!! = (2n + 1)(2n - 1)!!. So, (2n - 1)!! (2n + 1)!! ) = (2n - 1)!! * (2n + 1)!! = (2n + 1) ( (2n - 1)!! )^2 )

But this might not help. Alternatively, perhaps express the term as:

π * (-1)^n / [ (2n - 1)!! (2n + 1)!! ) ]

But this seems difficult to sum. Maybe there's a better approach.

Alternatively, perhaps consider changing variables in the original integral. Let me go back to the original integral:

∫_{0}^{2} cos(√(x(2 - x))) dx

We did substitution u = x - 1, leading to 2 ∫_{0}^{1} cos(√(1 - u²)) du. Let me consider polar coordinates. If we set u = sinθ, then √(1 - u²) = cosθ, and du = cosθ dθ. Wait, but we tried that earlier. Let me try again. Let u = sinθ, then when u=0, θ=0; u=1, θ=π/2. Then, the integral becomes ∫0^{π/2} cos(cosθ) * cosθ dθ. Hmm, but integrating cos(cosθ) * cosθ dθ. Not sure if that's a standard integral. Maybe expand cos(cosθ) in a Fourier series or Bessel functions.

Wait, recall that the integral of cos(a cosθ) cosθ dθ from 0 to π/2 is related to Bessel functions. Specifically, the Bessel function of the first kind J_1(a). Let me check. The integral representation of Bessel functions is J_n(x) = (1/π) ∫0^π cos(nθ - x sinθ) dθ. But not sure if that's applicable here. Alternatively, there's an integral involving cos(z cosθ) which is related to J_0(z). For example, ∫0^{π} cos(z cosθ) dθ = π J_0(z). But our integral is from 0 to π/2 and has an extra cosθ term. Let me see.

Alternatively, differentiate under the integral sign. Let me consider I(a) = ∫0^{π/2} cos(a cosθ) dθ. Then, dI/da = -∫0^{π/2} sin(a cosθ) sinθ dθ. But not sure. Alternatively, integrating by parts. Let me try integrating ∫ cos(cosθ) cosθ dθ. Let me set t = cosθ, then dt = -sinθ dθ. Hmm, but the integral becomes ∫ cos(t) * t * (-dt)/sqrt(1 - t²). From t=1 to t=0, so ∫0^1 [t cos(t) / sqrt(1 - t²)] dt. Wait, this is the same as the substitution we did earlier, leading to the same integral. So, this seems to circle back.

Alternatively, perhaps use the integrand's relation to Bessel functions. Let me recall that ∫0^π/2 cos(a cosθ) cosθ dθ. Let me check some integral tables or properties. Alternatively, expand cos(a cosθ) in a series. Let's use the expansion cos(z) = Σ_{k=0}^∞ (-1)^k z^{2k}/(2k)!). So, cos(a cosθ) = Σ_{k=0}^∞ (-1)^k (a cosθ)^{2k}/(2k)! ). Then, multiply by cosθ and integrate term by term:

∫0^{π/2} cos(a cosθ) cosθ dθ = Σ_{k=0}^∞ (-1)^k a^{2k}/(2k)! ) ∫0^{π/2} cos^{2k + 1}θ dθ.

But we already know that ∫0^{π/2} cos^{2k + 1}θ dθ = (sqrt(π)/2) Γ(k + 1)/Γ(k + 3/2). Which is similar to the previous expression. So, substituting back, this becomes Σ_{k=0}^∞ (-1)^k a^{2k}/(2k)! ) * (sqrt(π)/2) Γ(k + 1)/Γ(k + 3/2).

But this seems similar to the previous series. For a = 1, this would be the integral we need. But this series might not have a closed-form expression, which suggests that the original integral might not have an elementary closed-form solution. Therefore, perhaps the integral can only be expressed in terms of Bessel functions or other special functions, or it has to be evaluated numerically.

Alternatively, let me check if the original integral can be expressed in terms of Bessel functions. Let me recall that the integral ∫0^π cos(z cosθ) dθ = π J_0(z). But our integral is from 0 to π/2 and has an extra cosθ term. Let me see if there's a similar identity. 

Alternatively, consider differentiating the Bessel function integral. For example, d/dz [J_0(z)] = -J_1(z). But I'm not sure. Let me check:

The integral representation of J_n(z) is J_n(z) = (1/π) ∫0^π cos(nθ - z sinθ) dθ. For n=0, J_0(z) = (1/π) ∫0^π cos(z sinθ) dθ. But our integral is ∫0^{π/2} cos(z cosθ) cosθ dθ. Not directly matching. Maybe another approach.

Alternatively, consider changing variables. Let φ = π/2 - θ. Then, cosθ = sinφ, and the integral becomes ∫0^{π/2} cos(z sinφ) sinφ dφ. Which is similar to the integral for Bessel functions. Indeed, the integral ∫0^{π/2} cos(z sinφ) sinφ dφ is related to the Struve function or maybe the Anger-Weber functions, but I'm not sure. Alternatively, integrating by parts. Let me set u = sinφ, dv = cos(z sinφ) dφ. Then, du = cosφ dφ, v = ... Hmm, not helpful.

Alternatively, note that ∫0^{π/2} cos(z sinφ) sinφ dφ = (π/2) [J_1(z) + H_1(z)] where H is the Struve function. But I'm not certain. Alternatively, check integral tables. According to some references, ∫0^{π/2} cos(a cosθ) cosθ dθ = (π/2) [J_1(a) + H_1(a)]. But I need to verify this. If that's the case, then for a = 1, the integral becomes (π/2)[J_1(1) + H_1(1)]. But I'm not sure if this is correct. Alternatively, perhaps it's expressed differently.

Alternatively, use numerical integration. Since the integral might not have an elementary closed-form, perhaps the problem expects recognizing that and proceeding to compute it numerically. But the first step in the problem says to compute the integral analytically to obtain the exact answer. So, maybe there's a substitution or a trick I'm missing.

Wait, going back to the original substitution. The integral after substitution is 2 ∫0^1 cos(√(1 - u²)) du. Let me consider another substitution: let t = √(1 - u²). Then, t = sqrt(1 - u²) => t² = 1 - u² => u = sqrt(1 - t²). Then, du = (-t)/sqrt(1 - t²) dt. When u=0, t=1; u=1, t=0. So, the integral becomes 2 ∫1^0 cos(t) * (-t)/sqrt(1 - t²) dt = 2 ∫0^1 [t cos(t) / sqrt(1 - t²)] dt. This is the same integral as before. Hmm.

Alternatively, maybe use integration by parts on this integral. Let me set v = t, dv = dt, and dw = cos(t)/sqrt(1 - t²) dt. But integrating dw would be difficult. Alternatively, set u = sinθ, but that leads back to the same problem.

Alternatively, consider the substitution t = sinφ. Then, sqrt(1 - t²) = cosφ, dt = cosφ dφ. Then, the integral becomes ∫0^{π/2} [sinφ cos(sinφ) / cosφ] cosφ dφ = ∫0^{π/2} sinφ cos(sinφ) dφ. Which is ∫0^{π/2} sinφ cos(sinφ) dφ. Let me set x = sinφ, then dx = cosφ dφ. When φ=0, x=0; φ=π/2, x=1. So, the integral becomes ∫0^1 x cosx dx. Which is straightforward! Wait, that's a simple integral. Wait, let me check:

Wait, if t = sinφ, then φ goes from 0 to π/2, t from 0 to 1. Then, the integral ∫0^{π/2} sinφ cos(sinφ) dφ becomes ∫0^1 t cos(t) dt. Because when t = sinφ, then dt = cosφ dφ, and sinφ = t. So, the integral becomes ∫0^1 t cos(t) dt. Which is manageable. So, the original integral after substitution is 2 * ∫0^1 [t cos(t) / sqrt(1 - t²)] dt, but through substitution t = sinφ, this becomes 2 * ∫0^{π/2} sinφ cos(sinφ) dφ = 2 * ∫0^1 t cos(t) dt. Wait, but how?

Wait, let me retrace. The integral after substitution t = sqrt(1 - u²) was 2 * ∫0^1 [t cos(t) / sqrt(1 - t²)] dt. Then, if we set t = sinφ, then sqrt(1 - t²) = cosφ, dt = cosφ dφ. So, the integral becomes 2 * ∫0^{π/2} [sinφ cos(sinφ) / cosφ] * cosφ dφ = 2 * ∫0^{π/2} sinφ cos(sinφ) dφ. Then, substituting x = sinφ, dx = cosφ dφ, so when φ=0, x=0; φ=π/2, x=1. So, the integral becomes 2 * ∫0^1 x cos(x) dx. That's correct! So, finally, the original integral reduces to 2 * ∫0^1 x cos(x) dx. That's a breakthrough!

Now, compute ∫ x cos(x) dx. Integration by parts: let u = x, dv = cos(x) dx. Then, du = dx, v = sin(x). So, ∫x cosx dx = x sinx - ∫ sinx dx = x sinx + cosx + C. Evaluated from 0 to 1:

[1*sin(1) + cos(1)] - [0 + cos(0)] = sin(1) + cos(1) - 1.

Therefore, the original integral is 2*(sin(1) + cos(1) - 1). So, the exact answer is 2(sin(1) + cos(1) - 1).

Wait, that seems too straightforward. Let me verify the steps again to make sure I didn't make a mistake.

Original integral: u = x - 1, leading to 2 ∫0^1 cos(√(1 - u²)) du. Then, substitution t = sqrt(1 - u²), leading to 2 ∫0^1 [t cos(t) / sqrt(1 - t²)] dt. Then, substitution t = sinφ, leading to 2 ∫0^{π/2} sinφ cos(sinφ) dφ. Then, substitution x = sinφ, leading to 2 ∫0^1 x cosx dx. Then, integrating by parts gives 2*(sin(1) + cos(1) - 1). Yes, that seems correct.

So, the exact answer is 2(sin(1) + cos(1) - 1). Let me compute this numerically. Let's compute sin(1) and cos(1) where 1 is in radians.

sin(1) ≈ 0.8414709848

cos(1) ≈ 0.5403023059

So, sin(1) + cos(1) ≈ 0.8414709848 + 0.5403023059 ≈ 1.3817732907

Subtract 1: 1.3817732907 - 1 = 0.3817732907

Multiply by 2: 0.3817732907 * 2 ≈ 0.7635465814

Rounded to 10 decimal places: 0.7635465814

But let me check with a calculator to verify.

Alternatively, compute using more precise calculations:

sin(1) = 0.84147098480789650665250232163029899962256306079837

cos(1) = 0.54030230586813971740093660744297660373231042061792

Sum: 0.8414709848078965 + 0.5403023058681397 = 1.3817732906760362

Subtract 1: 0.3817732906760362

Multiply by 2: 0.7635465813520724

Rounded to 10 decimal places: 0.7635465814

So, the numerical approximation is approximately 0.7635465814.

Therefore, the exact answer is 2(sin(1) + cos(1) - 1), and the numerical value is approximately 0.7635465814.

But wait, let me check if the steps are correct. The key step was when we substituted t = sinφ in the integral ∫0^1 [t cos(t) / sqrt(1 - t²)] dt. Let me verify that substitution.

Let t = sinφ, so dt = cosφ dφ. Then, sqrt(1 - t²) = cosφ. So, the integral becomes ∫ [sinφ cos(sinφ) / cosφ] * cosφ dφ = ∫ sinφ cos(sinφ) dφ. Then, changing variable to x = sinφ, dx = cosφ dφ, so when φ=0, x=0; φ=π/2, x=1. So, the integral becomes ∫0^1 x cosx dx. Yes, that's correct. Therefore, the steps are valid.

Therefore, the exact answer is 2(sin(1) + cos(1) - 1), and the numerical approximation is approximately 0.7635465814.
</think>

{"answer": "2\\left(\\sin(1) + \\cos(1) - 1\\right)", "numerical_answer": "0.7635465814"}