We start with the integral

  I = ∫₀¹ [(1 – x^(25))^(1/20) – (1 – x^(20))^(1/25)] dx.

Step 1. Express each term in a form that involves a Beta integral. In general, one can show that
  ∫₀¹ (1 – x^m)^(p–1) dx = (1/m) · B(1/m, p),
where B(x, y) is the Beta function.

For the first term, write (1 – x^(25))^(1/20) as (1 – x^(25))^(p–1) with
  p – 1 = 1/20 ⟹ p = 1/20 + 1 = 21/20.
Thus,
  I₁ = ∫₀¹ (1 – x^(25))^(1/20) dx = 1/25 · B(1/25, 21/20).

Similarly, for the second term, (1 – x^(20))^(1/25) is written with
  p – 1 = 1/25 ⟹ p = 1/25 + 1 = 26/25.
Thus,
  I₂ = ∫₀¹ (1 – x^(20))^(1/25) dx = 1/20 · B(1/20, 26/25).

Hence, the original integral becomes:
  I = I₁ – I₂ = [1/25 · B(1/25, 21/20)] – [1/20 · B(1/20, 26/25)].

Step 2. Express each Beta function in terms of Gamma functions:
  B(x, y) = Γ(x) Γ(y) / Γ(x + y).

So we have:
  I₁ = (1/25) · [Γ(1/25) Γ(21/20)] / [Γ(1/25 + 21/20)],
  I₂ = (1/20) · [Γ(1/20) Γ(26/25)] / [Γ(1/20 + 26/25)].

Notice that
  1/25 + 21/20 = 1/20 + 26/25 = (4/100 + 105/100) = 109/100.
Thus, both terms have the same denominator Γ(109/100), and we write:
  I = 1/Γ(109/100) · [ (1/25) Γ(1/25) Γ(21/20) – (1/20) Γ(1/20) Γ(26/25) ].

Step 3. Use the Gamma function property:
  Γ(z+1) = z · Γ(z).

Since
  21/20 = 1/20 + 1 ⟹ Γ(21/20) = (1/20) Γ(1/20),
and
  26/25 = 1/25 + 1 ⟹ Γ(26/25) = (1/25) Γ(1/25),
we substitute to obtain:
  (1/25) Γ(1/25) Γ(21/20) = (1/25) Γ(1/25) · (1/20) Γ(1/20) = 1/(25·20) Γ(1/25) Γ(1/20)
and
  (1/20) Γ(1/20) Γ(26/25) = (1/20) Γ(1/20) · (1/25) Γ(1/25) = 1/(20·25) Γ(1/20) Γ(1/25).

Thus, both terms are identical and cancel:
  I = 1/Γ(109/100) · [1/(25·20) Γ(1/25) Γ(1/20) – 1/(25·20) Γ(1/25) Γ(1/20)] = 0.

Step 4. Conclude and provide the numerical value. Since I = 0 exactly, the numerical approximation is 0.0000000000 when rounded to 10 decimal places.

{"answer": "0", "numerical_answer": "0.0000000000"}