Let's solve the integral:
\[
I = \int_{0}^{2} x^{1/4} (2-x)^{-1/4} \cosh\left(1 \sqrt[4]{x(2-x)}\right) dx
\]

**Step 1: Substitution**

Let us use the substitution:
\[
x = 2 \sin^2 \theta, \quad \theta \in [0, \pi/2]
\]
Then,
\[
dx = 4 \sin\theta \cos\theta d\theta = 2 \sin 2\theta d\theta
\]
\[
x^{1/4} = (2 \sin^2\theta)^{1/4} = 2^{1/4} (\sin\theta)^{1/2}
\]
\[
2-x = 2 - 2\sin^2\theta = 2\cos^2\theta
\]
\[
(2-x)^{-1/4} = (2\cos^2\theta)^{-1/4} = 2^{-1/4} (\cos\theta)^{-1/2}
\]
\[
x(2-x) = 2\sin^2\theta \cdot 2\cos^2\theta = 4\sin^2\theta \cos^2\theta = (\sin 2\theta)^2
\]
\[
\sqrt[4]{x(2-x)} = \sqrt[4]{(\sin 2\theta)^2} = (\sin 2\theta)^{1/2}
\]

Now, substitute all into the integral:
\[
I = \int_{0}^{\pi/2} 2^{1/4} (\sin\theta)^{1/2} \cdot 2^{-1/4} (\cos\theta)^{-1/2} \cosh\left((\sin 2\theta)^{1/2}\right) \cdot 2\sin 2\theta d\theta
\]
\[
2^{1/4} \cdot 2^{-1/4} = 1
\]
\[
I = 2 \int_{0}^{\pi/2} (\sin\theta)^{1/2} (\cos\theta)^{-1/2} \cosh\left((\sin 2\theta)^{1/2}\right) \sin 2\theta d\theta
\]
But \(\sin 2\theta = 2\sin\theta \cos\theta\), so:
\[
I = 2 \int_{0}^{\pi/2} (\sin\theta)^{1/2} (\cos\theta)^{-1/2} \cosh\left((\sin 2\theta)^{1/2}\right) \cdot 2\sin\theta \cos\theta d\theta
\]
\[
= 4 \int_{0}^{\pi/2} (\sin\theta)^{3/2} (\cos\theta)^{1/2} \cosh\left((\sin 2\theta)^{1/2}\right) d\theta
\]

**Step 2: Further Substitution**

Let us try to simplify further. Let \(u = \sin 2\theta\), so as \(\theta\) goes from \(0\) to \(\pi/2\), \(u\) goes from \(0\) to \(1\).

Recall:
\[
\sin 2\theta = 2\sin\theta\cos\theta \implies \sin\theta\cos\theta = \frac{u}{2}
\]
Also,
\[
d\theta = \frac{du}{2\cos 2\theta}
\]
But,
\[
\sin\theta = \sqrt{\frac{1 - \cos 2\theta}{2}}, \quad \cos\theta = \sqrt{\frac{1 + \cos 2\theta}{2}}
\]
But this seems to complicate the integral.

Alternatively, let's try to expand the \(\cosh\) function:
\[
\cosh(z) = \sum_{n=0}^{\infty} \frac{z^{2n}}{(2n)!}
\]
So,
\[
\cosh\left((\sin 2\theta)^{1/2}\right) = \sum_{n=0}^{\infty} \frac{(\sin 2\theta)^n}{(2n)!}
\]

Therefore,
\[
I = 4 \int_{0}^{\pi/2} (\sin\theta)^{3/2} (\cos\theta)^{1/2} \sum_{n=0}^{\infty} \frac{(\sin 2\theta)^n}{(2n)!} d\theta
\]
\[
= 4 \sum_{n=0}^{\infty} \frac{1}{(2n)!} \int_{0}^{\pi/2} (\sin\theta)^{3/2} (\cos\theta)^{1/2} (\sin 2\theta)^n d\theta
\]
But \(\sin 2\theta = 2\sin\theta\cos\theta\), so
\[
(\sin 2\theta)^n = 2^n (\sin\theta)^n (\cos\theta)^n
\]
So,
\[
I = 4 \sum_{n=0}^{\infty} \frac{2^n}{(2n)!} \int_{0}^{\pi/2} (\sin\theta)^{3/2 + n} (\cos\theta)^{1/2 + n} d\theta
\]

But
\[
\int_{0}^{\pi/2} (\sin\theta)^{a-1} (\cos\theta)^{b-1} d\theta = \frac{1}{2} B\left(\frac{a}{2}, \frac{b}{2}\right)
\]
where \(B(x, y)\) is the Beta function.

Here,
\[
a = \frac{5}{2} + n, \quad b = \frac{3}{2} + n
\]
So,
\[
I = 4 \sum_{n=0}^{\infty} \frac{2^n}{(2n)!} \cdot \frac{1}{2} B\left(\frac{5/2 + n}{2}, \frac{3/2 + n}{2}\right)
\]
\[
= 2 \sum_{n=0}^{\infty} \frac{2^n}{(2n)!} B\left(\frac{5 + 2n}{4}, \frac{3 + 2n}{4}\right)
\]

Recall that
\[
B(x, y) = \frac{\Gamma(x)\Gamma(y)}{\Gamma(x+y)}
\]

So,
\[
I = 2 \sum_{n=0}^{\infty} \frac{2^n}{(2n)!} \frac{\Gamma\left(\frac{5 + 2n}{4}\right) \Gamma\left(\frac{3 + 2n}{4}\right)}{\Gamma\left(\frac{5 + 2n}{4} + \frac{3 + 2n}{4}\right)}
\]
\[
= 2 \sum_{n=0}^{\infty} \frac{2^n}{(2n)!} \frac{\Gamma\left(\frac{5 + 2n}{4}\right) \Gamma\left(\frac{3 + 2n}{4}\right)}{\Gamma\left(2 + n\right)}
\]

**Step 3: Final Exact Answer**

Thus, the exact answer is:
\[
I = 2 \sum_{n=0}^{\infty} \frac{2^n}{(2n)!} \frac{\Gamma\left(\frac{5 + 2n}{4}\right) \Gamma\left(\frac{3 + 2n}{4}\right)}{\Gamma(2 + n)}
\]

**Step 4: Numerical Approximation**

Let us compute the first few terms numerically:

- For \(n=0\):
  \[
  \frac{2^0}{0!} \frac{\Gamma(5/4)\Gamma(3/4)}{\Gamma(2)}
  \]
  \(\Gamma(2) = 1\), \(\Gamma(5/4) \approx 0.9064024771\), \(\Gamma(3/4) \approx 1.225416703\)
  So,
  \[
  2 \times 0.9064024771 \times 1.225416703 \approx 2 \times 1.110720734 \approx 2.221441468
  \]

- For \(n=1\):
  \[
  \frac{2^1}{2!} \frac{\Gamma(7/4)\Gamma(5/4)}{\Gamma(3)}
  \]
  \(\Gamma(3) = 2\), \(\Gamma(7/4) \approx 1.225416703\), \(\Gamma(5/4) \approx 0.9064024771\)
  \[
  \frac{2}{2} \frac{1.225416703 \times 0.9064024771}{2} = \frac{1.110720734}{2} = 0.555360367
  \]
  Multiply by 2: \(2 \times 0.555360367 = 1.110720734\)

- For \(n=2\):
  \[
  \frac{2^2}{4!} \frac{\Gamma(9/4)\Gamma(7/4)}{\Gamma(4)}
  \]
  \(2^2 = 4\), \(4! = 24\), \(\Gamma(4) = 6\)
  \(\Gamma(9/4) \approx 1.133003096\), \(\Gamma(7/4) \approx 1.225416703\)
  \[
  \frac{4}{24} \frac{1.133003096 \times 1.225416703}{6} = \frac{1}{6} \frac{1.388129438}{6} = \frac{1.388129438}{36} \approx 0.038559151
  \]
  Multiply by 2: \(2 \times 0.038559151 = 0.077118302\)

- For \(n=3\):
  \[
  \frac{2^3}{6!} \frac{\Gamma(11/4)\Gamma(9/4)}{\Gamma(5)}
  \]
  \(2^3 = 8\), \(6! = 720\), \(\Gamma(5) = 24\)
  \(\Gamma(11/4) \approx 1.412697\), \(\Gamma(9/4) \approx 1.133003096\)
  \[
  \frac{8}{720} \frac{1.412697 \times 1.133003096}{24} = \frac{1}{90} \frac{1.601086}{24} = \frac{1.601086}{2160} \approx 0.000741242
  \]
  Multiply by 2: \(2 \times 0.000741242 = 0.001482484\)

Sum up the first four terms:
\[
2.221441468 + 1.110720734 + 0.077118302 + 0.001482484 \approx 3.410762988
\]

The series converges rapidly. Adding a few more terms (which are much smaller), the sum approaches approximately \(3.410763\).

**Step 5: JSON Output**

```json
{"answer": "2 \\sum_{n=0}^{\\infty} \\frac{2^n}{(2n)!} \\frac{\\Gamma\\left(\\frac{5+2n}{4}\\right) \\Gamma\\left(\\frac{3+2n}{4}\\right)}{\\Gamma(2+n)}", "numerical_answer": "3.4107629882"}
```