To solve the definite integral \(\int_{0}^{1} \arcsin(x) \arccos(x) \, dx\), we will follow the steps outlined:

### Step 1: Analytical Computation

First, we use the identity \(\arcsin(x) + \arccos(x) = \frac{\pi}{2}\) for \(x \in [0, 1]\). This allows us to rewrite the integrand:

\[
\arcsin(x) \arccos(x) = \arcsin(x) \left( \frac{\pi}{2} - \arcsin(x) \right)
\]

Thus, the integral becomes:

\[
\int_{0}^{1} \arcsin(x) \arccos(x) \, dx = \int_{0}^{1} \arcsin(x) \left( \frac{\pi}{2} - \arcsin(x) \right) \, dx
\]

Expanding the integrand:

\[
\int_{0}^{1} \arcsin(x) \left( \frac{\pi}{2} - \arcsin(x) \right) \, dx = \frac{\pi}{2} \int_{0}^{1} \arcsin(x) \, dx - \int_{0}^{1} \arcsin^2(x) \, dx
\]

We now need to evaluate these two integrals separately.

#### Integral 1: \(\int_{0}^{1} \arcsin(x) \, dx\)

Using integration by parts, let \(u = \arcsin(x)\) and \(dv = dx\). Then \(du = \frac{1}{\sqrt{1 - x^2}} \, dx\) and \(v = x\). Applying integration by parts:

\[
\int \arcsin(x) \, dx = x \arcsin(x) - \int \frac{x}{\sqrt{1 - x^2}} \, dx
\]

The remaining integral can be solved by substitution. Let \(t = 1 - x^2\), then \(dt = -2x \, dx\):

\[
\int \frac{x}{\sqrt{1 - x^2}} \, dx = -\frac{1}{2} \int \frac{1}{\sqrt{t}} \, dt = -\sqrt{t} = -\sqrt{1 - x^2}
\]

Thus:

\[
\int \arcsin(x) \, dx = x \arcsin(x) + \sqrt{1 - x^2} + C
\]

Evaluating from 0 to 1:

\[
\int_{0}^{1} \arcsin(x) \, dx = \left[ x \arcsin(x) + \sqrt{1 - x^2} \right]_{0}^{1} = \left( 1 \cdot \frac{\pi}{2} + 0 \right) - \left( 0 + 1 \right) = \frac{\pi}{2} - 1
\]

#### Integral 2: \(\int_{0}^{1} \arcsin^2(x) \, dx\)

This integral is more complex. We use the series expansion for \(\arcsin(x)\):

\[
\arcsin(x) = \sum_{n=0}^{\infty} \frac{(2n)!}{4^n (n!)^2 (2n+1)} x^{2n+1}
\]

Squaring this series and integrating term-by-term is cumbersome. Instead, we use a known result:

\[
\int_{0}^{1} \arcsin^2(x) \, dx = \frac{\pi^2}{8} - 1
\]

### Step 2: Combine the Results

Combining the results from the two integrals:

\[
\int_{0}^{1} \arcsin(x) \arccos(x) \, dx = \frac{\pi}{2} \left( \frac{\pi}{2} - 1 \right) - \left( \frac{\pi^2}{8} - 1 \right)
\]

Simplifying:

\[
\frac{\pi^2}{4} - \frac{\pi}{2} - \frac{\pi^2}{8} + 1 = \frac{\pi^2}{8} - \frac{\pi}{2} + 1
\]

### Step 3: Numerical Approximation

Using \(\pi \approx 3.141592653589793\):

\[
\frac{\pi^2}{8} \approx \frac{9.869604401089358}{8} \approx 1.2337005501361698
\]

\[
\frac{\pi}{2} \approx 1.5707963267948966
\]

\[
\frac{\pi^2}{8} - \frac{\pi}{2} + 1 \approx 1.2337005501361698 - 1.5707963267948966 + 1 \approx 0.6629042233412732
\]

### Step 4: Final Answer in JSON Format

\[
\boxed{
\begin{aligned}
\text{"answer": "}\frac{\pi^2}{8} - \frac{\pi}{2} + 1\text{"}, \\
\text{"numerical_answer": "0.6629042233"}
\end{aligned}
}
\]