To solve the definite integral \(\int\limits_0^1 x \ln\frac{1+\sqrt{1-x^2}}{1-\sqrt{1-x^2}} I_0(2x) \, dx\), we will follow the steps outlined:

### Step 1: Analytical Computation

First, let's rewrite the integral for clarity:
\[ I = \int_0^1 x \ln\left(\frac{1+\sqrt{1-x^2}}{1-\sqrt{1-x^2}}\right) I_0(2x) \, dx \]

We recognize that the argument of the logarithm can be simplified using the hyperbolic identity:
\[ \ln\left(\frac{1+\sqrt{1-x^2}}{1-\sqrt{1-x^2}}\right) = 2 \tanh^{-1}\left(\sqrt{1-x^2}\right) \]

Thus, the integral becomes:
\[ I = 2 \int_0^1 x \tanh^{-1}\left(\sqrt{1-x^2}\right) I_0(2x) \, dx \]

Next, we use the series expansion for the modified Bessel function of the first kind \(I_0(2x)\):
\[ I_0(2x) = \sum_{n=0}^\infty \frac{(x^2)^n}{(n!)^2} \]

Substituting this into the integral, we get:
\[ I = 2 \int_0^1 x \tanh^{-1}\left(\sqrt{1-x^2}\right) \sum_{n=0}^\infty \frac{(x^2)^n}{(n!)^2} \, dx \]

Interchanging the sum and the integral (justified by uniform convergence), we have:
\[ I = 2 \sum_{n=0}^\infty \frac{1}{(n!)^2} \int_0^1 x^{2n+1} \tanh^{-1}\left(\sqrt{1-x^2}\right) \, dx \]

Now, we need to evaluate the integral:
\[ \int_0^1 x^{2n+1} \tanh^{-1}\left(\sqrt{1-x^2}\right) \, dx \]

Using the substitution \( t = \sqrt{1-x^2} \), we get \( dt = -\frac{x}{\sqrt{1-x^2}} dx \) and \( x = \sqrt{1-t^2} \). The limits change from \( x = 0 \) to \( t = 1 \) and from \( x = 1 \) to \( t = 0 \). Thus, the integral becomes:
\[ \int_0^1 x^{2n+1} \tanh^{-1}\left(\sqrt{1-x^2}\right) \, dx = \int_1^0 (1-t^2)^{n+\frac{1}{2}} \tanh^{-1}(t) \left(-\frac{t}{\sqrt{1-t^2}}\right) dt \]
\[ = \int_0^1 (1-t^2)^{n+\frac{1}{2}} \tanh^{-1}(t) \frac{t}{\sqrt{1-t^2}} dt \]
\[ = \int_0^1 (1-t^2)^n t \tanh^{-1}(t) \, dt \]

This integral is known to be:
\[ \int_0^1 (1-t^2)^n t \tanh^{-1}(t) \, dt = \frac{1}{2(n+1)} \]

Thus, the integral simplifies to:
\[ I = 2 \sum_{n=0}^\infty \frac{1}{(n!)^2} \cdot \frac{1}{2(n+1)} = \sum_{n=0}^\infty \frac{1}{(n!)^2 (n+1)} \]

This series is known to sum to:
\[ \sum_{n=0}^\infty \frac{1}{(n!)^2 (n+1)} = \frac{e^2 - 1}{2} \]

### Step 2: Numerical Approximation

To find the numerical approximation, we evaluate:
\[ \frac{e^2 - 1}{2} \approx \frac{7.38905609893065 - 1}{2} \approx \frac{6.38905609893065}{2} \approx 3.194528049465325 \]

### Step 3: Final Answer in JSON Format

```json
{"answer": "\\frac{e^2 - 1}{2}", "numerical_answer": "3.1945280495"}
```