To solve the definite integral \(\int\limits_{0}^{1}\arcsin\left(0.5\sqrt{x(1-x)}\right)dx\), we will follow these steps:

### Step 1: Simplify the Integrand
Let’s denote the integrand as:
\[
I = \arcsin\left(\frac{1}{2}\sqrt{x(1-x)}\right)
\]
We can make a substitution to simplify the expression inside the arcsine. Let:
\[
x = \sin^2\theta \quad \Rightarrow \quad dx = 2\sin\theta\cos\theta \, d\theta
\]
The limits change as follows:
- When \(x = 0\), \(\theta = 0\)
- When \(x = 1\), \(\theta = \frac{\pi}{2}\)

Substituting into the integrand:
\[
\sqrt{x(1-x)} = \sqrt{\sin^2\theta(1 - \sin^2\theta)} = \sin\theta\cos\theta
\]
Thus:
\[
I = \arcsin\left(\frac{1}{2}\sin\theta\cos\theta\right)
\]

### Step 2: Simplify the Argument of Arcsine
Recall the double-angle identity:
\[
\sin\theta\cos\theta = \frac{1}{2}\sin(2\theta)
\]
So:
\[
I = \arcsin\left(\frac{1}{4}\sin(2\theta)\right)
\]

### Step 3: Change of Variables
Let’s set:
\[
u = 2\theta \quad \Rightarrow \quad d\theta = \frac{du}{2}
\]
The limits become:
- When \(\theta = 0\), \(u = 0\)
- When \(\theta = \frac{\pi}{2}\), \(u = \pi\)

The integral becomes:
\[
\int_{0}^{\pi} \arcsin\left(\frac{1}{4}\sin u\right) \cdot \frac{du}{2}
\]

### Step 4: Exploit Symmetry
The integrand is symmetric about \(u = \frac{\pi}{2}\), so we can write:
\[
\int_{0}^{\pi} \arcsin\left(\frac{1}{4}\sin u\right) du = 2 \int_{0}^{\frac{\pi}{2}} \arcsin\left(\frac{1}{4}\sin u\right) du
\]
Thus, the integral simplifies to:
\[
\int_{0}^{\frac{\pi}{2}} \arcsin\left(\frac{1}{4}\sin u\right) du
\]

### Step 5: Series Expansion of Arcsine
For \(|z| \leq 1\), the Taylor series for \(\arcsin(z)\) is:
\[
\arcsin(z) = \sum_{n=0}^{\infty} \frac{(2n)!}{4^n (n!)^2 (2n+1)} z^{2n+1}
\]
Applying this to our integrand:
\[
\arcsin\left(\frac{1}{4}\sin u\right) = \sum_{n=0}^{\infty} \frac{(2n)!}{4^n (n!)^2 (2n+1)} \left(\frac{1}{4}\sin u\right)^{2n+1}
\]
Thus, the integral becomes:
\[
\sum_{n=0}^{\infty} \frac{(2n)!}{4^n (n!)^2 (2n+1)} \left(\frac{1}{4}\right)^{2n+1} \int_{0}^{\frac{\pi}{2}} \sin^{2n+1} u \, du
\]

### Step 6: Evaluate the Integral of \(\sin^{2n+1} u\)
The integral:
\[
\int_{0}^{\frac{\pi}{2}} \sin^{2n+1} u \, du = \frac{\sqrt{\pi} \, \Gamma(n+1)}{2 \, \Gamma\left(n + \frac{3}{2}\right)}
\]
Using the identity \(\Gamma\left(n + \frac{3}{2}\right) = \frac{(2n+1)!!}{2^{n+1}} \sqrt{\pi}\), we get:
\[
\int_{0}^{\frac{\pi}{2}} \sin^{2n+1} u \, du = \frac{2^{2n} (n!)^2}{(2n+1)!}
\]

### Step 7: Substitute Back into the Series
Substituting this result back:
\[
\sum_{n=0}^{\infty} \frac{(2n)!}{4^n (n!)^2 (2n+1)} \left(\frac{1}{4}\right)^{2n+1} \cdot \frac{2^{2n} (n!)^2}{(2n+1)!}
\]
Simplifying:
\[
\sum_{n=0}^{\infty} \frac{1}{(2n+1)^2} \left(\frac{1}{4}\right)^{2n+1}
\]

### Step 8: Recognize the Series
This series can be expressed in terms of the polylogarithm function \(\text{Li}_2(z)\):
\[
\sum_{n=0}^{\infty} \frac{z^{2n+1}}{(2n+1)^2} = \frac{1}{2} \left(\text{Li}_2(z) - \text{Li}_2(-z)\right)
\]
For \(z = \frac{1}{4}\):
\[
\sum_{n=0}^{\infty} \frac{1}{(2n+1)^2} \left(\frac{1}{4}\right)^{2n+1} = \frac{1}{2} \left(\text{Li}_2\left(\frac{1}{4}\right) - \text{Li}_2\left(-\frac{1}{4}\right)\right)
\]

### Step 9: Numerical Approximation
Using known values of the dilogarithm:
\[
\text{Li}_2\left(\frac{1}{4}\right) \approx 0.2676526390
\]
\[
\text{Li}_2\left(-\frac{1}{4}\right) \approx -0.2359002970
\]
Thus:
\[
\frac{1}{2} \left(0.2676526390 - (-0.2359002970)\right) = \frac{1}{2} \times 0.5035529360 = 0.2517764680
\]

### Final Answer
The exact answer involves the dilogarithm function, and the numerical approximation is:
\[
0.2517764680
\]

```json
{"answer": "\\frac{1}{2} \\left(\\text{Li}_2\\left(\\frac{1}{4}\\right) - \\text{Li}_2\\left(-\\frac{1}{4}\\right)\\right)", "numerical_answer": "0.2517764680"}
```