We wish to evaluate

  I = ∫ from -1 to 1 [cos x / (1 + e^(–1/x))] dx.

Step 1. Recognize symmetry:
Define
  f(x) = cos x/(1 + e^(–1/x)).
Notice that cos x is an even function. Now compute f(–x):
  f(–x) = cos(–x)/(1 + e^(–1/(–x)))
      = cos x/(1 + e^(1/x))  (since cos(–x)=cos x).

Step 2. Sum f(x) and f(–x):
  f(x) + f(–x) = cos x/(1 + e^(–1/x)) + cos x/(1 + e^(1/x))
Factor out cos x:
  = cos x [1/(1 + e^(–1/x)) + 1/(1 + e^(1/x))].

Now, observe that
  1/(1 + e^(–1/x)) = e^(1/x)/(e^(1/x) + 1)
so we have:
  1/(1 + e^(–1/x)) + 1/(1 + e^(1/x)) = e^(1/x)/(1 + e^(1/x)) + 1/(1 + e^(1/x)) = (e^(1/x) + 1)/(1 + e^(1/x)) = 1.

Thus, the sum simplifies to:
  f(x) + f(–x) = cos x.

Step 3. Use the symmetry in the integral:
Notice that the interval [–1, 1] is symmetric, so if we add the integrals of f(x) and f(–x), we get:
  ∫₋₁¹ f(x) dx + ∫₋₁¹ f(–x) dx = ∫₋₁¹ cos x dx.
But by substitution, the two integrals on the left are equal. In other words, letting u = – x in the second integral shows that:
  2 ∫₋₁¹ f(x) dx = ∫₋₁¹ cos x dx.
Therefore,
  ∫₋₁¹ f(x) dx = (1/2) ∫₋₁¹ cos x dx.

Step 4. Evaluate ∫₋₁¹ cos x dx:
Since cos x is even:
  ∫₋₁¹ cos x dx = 2∫₀¹ cos x dx = 2[sin x]₀¹ = 2 sin 1.

Thus, the original integral becomes:
  I = ∫₋₁¹ f(x) dx = (1/2) (2 sin 1) = sin 1.

Step 5. Numerical approximation:
  sin 1 (with 1 in radians) ≈ 0.8414709848 (rounded to 10 decimal places).

Final Answer in JSON format:
{"answer": "$\\sin(1)$", "numerical_answer": "0.8414709848"}