Let us consider the integral:
\[
I = \int_0^1 \frac{1}{1 + x^2} \arctan\left(x^{11+\sqrt{120}}\right) dx
\]

### Step 1: Let \( \alpha = 11 + \sqrt{120} \)
So the integral is:
\[
I = \int_0^1 \frac{1}{1 + x^2} \arctan(x^{\alpha}) dx
\]

### Step 2: Use substitution and symmetry of the integral

Let us try the substitution \( x \mapsto 1/x \):

Let \( x = \tan\theta \), \( dx = \sec^2\theta d\theta \):
- As \( x \) goes from \( 0 \) to \( 1 \), \( \theta \) goes from \( 0 \) to \( \pi/4 \).
- \( 1+x^2 = 1+\tan^2\theta = \sec^2\theta \)
- \( x^{\alpha} = \tan^{\alpha}\theta \)

The integral becomes:
\[
I = \int_0^1 \frac{1}{1 + x^2} \arctan(x^{\alpha}) dx
  = \int_{\theta=0}^{\theta=\pi/4} \arctan(\tan^\alpha\theta) d\theta
\]

So we have reduced the integral to:
\[
I = \int_0^{\pi/4} \arctan(\tan^\alpha\theta) d\theta
\]

### Step 3: Use a property of the integral

Let’s evaluate \( J(\alpha) = \int_0^{\pi/4} \arctan(\tan^\alpha\theta) d\theta \).

Let’s make the substitution \( \theta \to \frac{\pi}{4} - \theta \):

- Then \( \tan(\frac{\pi}{4}-\theta) = \frac{1-\tan\theta}{1+\tan\theta} \), but maybe that's not making it simpler.

Alternatively, note that:
\[
\tan^\alpha\theta = [\tan\theta]^\alpha
\]
and
\[
\arctan(\tan^\alpha\theta) + \arctan(\cot^\alpha\theta) = \frac{\pi}{2}
\]
when \( \theta \in (0, \pi/4) \), because \( \cot^\alpha\theta = \tan^\alpha(\pi/2-\theta) \), and so over \( \theta \in (0, \pi/4) \) this applies.

So, let's write:
\[
J(\alpha) + J(-\alpha) = \int_0^{\pi/4} \left[ \arctan(\tan^\alpha\theta) + \arctan(\tan^{-\alpha}\theta) \right] d\theta
\]

But \( \arctan(\tan^{-\alpha}\theta) = \arctan(\cot^\alpha\theta) \), so over \( (0, \pi/4) \):

\[
\arctan(\tan^\alpha\theta) + \arctan(\cot^\alpha\theta) = \frac{\pi}{2}
\]
Hence,
\[
J(\alpha) + J(-\alpha) = \int_0^{\pi/4} \frac{\pi}{2} d\theta = \frac{\pi}{2} \cdot \frac{\pi}{4} = \frac{\pi^2}{8}
\]
Now, note that for positive \(\alpha\),
\[
J(\alpha) = J(-\alpha)
\]
because:
\[
\arctan(\tan^{-\alpha}\theta) = \arctan(\cot^\alpha\theta) = \frac{\pi}{2} - \arctan(\tan^\alpha\theta)
\]
But unless \(\tan^\alpha\theta\) is positive and monotonically increasing, care must be taken.

In any case, as \(\alpha > 0\), for \( \theta \in (0, \pi/4) \), \( 0 \leq \tan\theta \leq 1 \), and so \( 0 \leq \tan^\alpha\theta \leq 1 \). Thus \( 0 \leq \arctan(\tan^\alpha\theta) \leq \pi/4 \).

### Step 4: Compute the complementary value

Alternatively, let’s evaluate
\[
J(\alpha) + J(-\alpha) = \frac{\pi^2}{8}
\]
Hence,
\[
J(\alpha) = J(-\alpha) = \frac{\pi^2}{16}
\]

So:
\[
I = \int_0^{\pi/4} \arctan(\tan^\alpha\theta) d\theta = \frac{\pi^2}{16}
\]

### Step 5: Numerical evaluation

\[
\frac{\pi^2}{16} = \frac{(3.141592653589793)^2}{16} = \frac{9.869604401089358}{16} = 0.616850275067085
\]

Rounded to 10 decimal places:  
\( 0.6168502751 \)

---

Final answer in requested JSON format:
```json
{"answer": "\\frac{\\pi^2}{16}", "numerical_answer": "0.6168502751"}
```