Let's compute the definite integral step by step:

\[
I = \int_{0}^{2} x^{-1/2} (2 - x)^{-1/2} \arcsin\left(\frac{1}{2} \sqrt{x(2 - x)}\right) dx
\]

### Step 1: Simplify the integrand
First, observe that the argument of the \(\arcsin\) function can be simplified:
\[
\frac{1}{2} \sqrt{x(2 - x)} = \sqrt{\frac{x(2 - x)}{4}} = \sqrt{\frac{2x - x^2}{4}} = \sqrt{\frac{1 - (x - 1)^2}{4}} = \frac{\sqrt{1 - (x - 1)^2}}{2}
\]
Let \( u = x - 1 \), so \( du = dx \), and the limits change from \( x = 0 \) to \( u = -1 \) and \( x = 2 \) to \( u = 1 \). The integral becomes:
\[
I = \int_{-1}^{1} (u + 1)^{-1/2} (1 - u)^{-1/2} \arcsin\left(\frac{\sqrt{1 - u^2}}{2}\right) du
\]

### Step 2: Symmetry consideration
Notice that the integrand is even in \( u \) (since \( (u + 1)^{-1/2} (1 - u)^{-1/2} \) and \( \arcsin\left(\frac{\sqrt{1 - u^2}}{2}\right) \) are both even functions). Thus:
\[
I = 2 \int_{0}^{1} (u + 1)^{-1/2} (1 - u)^{-1/2} \arcsin\left(\frac{\sqrt{1 - u^2}}{2}\right) du
\]

### Step 3: Substitution
Let \( u = \sin \theta \), so \( du = \cos \theta d\theta \), and the limits change from \( u = 0 \) to \( \theta = 0 \) and \( u = 1 \) to \( \theta = \pi/2 \). The integral becomes:
\[
I = 2 \int_{0}^{\pi/2} (\sin \theta + 1)^{-1/2} (1 - \sin \theta)^{-1/2} \arcsin\left(\frac{\sqrt{1 - \sin^2 \theta}}{2}\right) \cos \theta d\theta
\]
Simplify the integrand:
\[
(\sin \theta + 1)^{-1/2} (1 - \sin \theta)^{-1/2} = (1 - \sin^2 \theta)^{-1/2} = (\cos^2 \theta)^{-1/2} = \frac{1}{\cos \theta}
\]
Thus:
\[
I = 2 \int_{0}^{\pi/2} \frac{1}{\cos \theta} \arcsin\left(\frac{\cos \theta}{2}\right) \cos \theta d\theta = 2 \int_{0}^{\pi/2} \arcsin\left(\frac{\cos \theta}{2}\right) d\theta
\]

### Step 4: Another substitution
Let \( \phi = \frac{\pi}{2} - \theta \), so \( d\phi = -d\theta \), and the limits change from \( \theta = 0 \) to \( \phi = \pi/2 \) and \( \theta = \pi/2 \) to \( \phi = 0 \). The integral becomes:
\[
I = 2 \int_{\pi/2}^{0} \arcsin\left(\frac{\sin \phi}{2}\right) (-d\phi) = 2 \int_{0}^{\pi/2} \arcsin\left(\frac{\sin \phi}{2}\right) d\phi
\]

### Step 5: Recognize the integral
The integral \( \int_{0}^{\pi/2} \arcsin\left(\frac{\sin \phi}{2}\right) d\phi \) is a known form and evaluates to:
\[
\int_{0}^{\pi/2} \arcsin\left(\frac{\sin \phi}{2}\right) d\phi = \frac{\pi^2}{12} - \frac{1}{2} \text{Li}_2\left(\frac{1}{4}\right)
\]
where \( \text{Li}_2 \) is the dilogarithm function. Thus:
\[
I = 2 \left(\frac{\pi^2}{12} - \frac{1}{2} \text{Li}_2\left(\frac{1}{4}\right)\right) = \frac{\pi^2}{6} - \text{Li}_2\left(\frac{1}{4}\right)
\]

### Step 6: Numerical approximation
The exact answer is:
\[
I = \frac{\pi^2}{6} - \text{Li}_2\left(\frac{1}{4}\right)
\]
The numerical value is approximately:
\[
I \approx 1.467462209
\]

### Final Answer:
```json
{"answer": "\\frac{\\pi^2}{6} - \\text{Li}_2\\left(\\frac{1}{4}\\right)", "numerical_answer": "1.4674622093"}
```