To solve the definite integral 

\[
\int_{420}^{1672} \frac{\sqrt{\ln(2023 - x)}}{\sqrt{\ln(2023 - x)} + \sqrt{\ln(x - 69)}} \, dx,
\]

we will follow these steps:

### Step 1: Symmetry and Substitution
First, observe the symmetry in the integral. Let’s perform a substitution to simplify the integrand. Let:

\[
a = 420, \quad b = 1672, \quad c = 2023, \quad d = 69.
\]

The integral becomes:

\[
I = \int_{a}^{b} \frac{\sqrt{\ln(c - x)}}{\sqrt{\ln(c - x)} + \sqrt{\ln(x - d)}} \, dx.
\]

Now, let’s make the substitution \( x = c + d - t \). Then:

- When \( x = a \), \( t = c + d - a \).
- When \( x = b \), \( t = c + d - b \).
- \( dx = -dt \).

The integral transforms as:

\[
I = \int_{c + d - a}^{c + d - b} \frac{\sqrt{\ln(t - d)}}{\sqrt{\ln(t - d)} + \sqrt{\ln(c - t)}} \, (-dt) = \int_{c + d - b}^{c + d - a} \frac{\sqrt{\ln(t - d)}}{\sqrt{\ln(t - d)} + \sqrt{\ln(c - t)}} \, dt.
\]

Now, notice that \( c + d - a = 2023 + 69 - 420 = 1672 \) and \( c + d - b = 2023 + 69 - 1672 = 420 \). Thus:

\[
I = \int_{420}^{1672} \frac{\sqrt{\ln(t - 69)}}{\sqrt{\ln(t - 69)} + \sqrt{\ln(2023 - t)}} \, dt.
\]

### Step 2: Adding the Original and Transformed Integrals
Now, add the original integral \( I \) and the transformed integral:

\[
2I = \int_{420}^{1672} \left( \frac{\sqrt{\ln(2023 - x)}}{\sqrt{\ln(2023 - x)} + \sqrt{\ln(x - 69)}} + \frac{\sqrt{\ln(x - 69)}}{\sqrt{\ln(x - 69)} + \sqrt{\ln(2023 - x)}} \right) dx.
\]

Simplify the integrand:

\[
\frac{\sqrt{\ln(2023 - x)} + \sqrt{\ln(x - 69)}}{\sqrt{\ln(2023 - x)} + \sqrt{\ln(x - 69)}} = 1.
\]

Thus:

\[
2I = \int_{420}^{1672} 1 \, dx = 1672 - 420 = 1252.
\]

Therefore:

\[
I = \frac{1252}{2} = 626.
\]

### Step 3: Numerical Approximation
The exact answer is \( 626 \), and its numerical approximation is:

\[
626.0000000000.
\]

### Final Answer
```json
{"answer": "626", "numerical_answer": "626.0000000000"}
```