To evaluate the definite integral

$$
\int_0^1 \mathbf{L}_0(2\sqrt{x}) \, \mathbf{E}\left(\sqrt{1 - x}\right) \, dx,
$$

we proceed by analyzing the structure of the integrand and leveraging known series expansions of the modified Struve function $\mathbf{L}_0(z)$ and the complete elliptic integral of the second kind $\mathbf{E}(k)$.

---

### **Step 1: Series Expansion of the Modified Struve Function**

The modified Struve function of order zero has the series representation:

$$
\mathbf{L}_0(z) = \frac{z}{2} \sum_{k=0}^{\infty} \frac{(z^2/4)^k}{\Gamma(k + 3/2)^2}.
$$

Substituting $ z = 2\sqrt{x} $, we obtain:

$$
\mathbf{L}_0(2\sqrt{x}) = \sqrt{x} \sum_{k=0}^{\infty} \frac{x^k}{\Gamma(k + 3/2)^2}.
$$

---

### **Step 2: Series Expansion of the Elliptic Integral**

The complete elliptic integral of the second kind has the hypergeometric representation:

$$
\mathbf{E}(k) = \frac{\pi}{2} \sum_{n=0}^{\infty} \frac{(-1/2)_n (1/2)_n}{(1)_n n!} k^{2n},
$$

where $(a)_n$ is the Pochhammer symbol (rising factorial). Substituting $ k = \sqrt{1 - x} $, we get:

$$
\mathbf{E}(\sqrt{1 - x}) = \frac{\pi}{2} \sum_{n=0}^{\infty} \frac{(-1/2)_n (1/2)_n}{(1)_n n!} (1 - x)^n.
$$

---

### **Step 3: Multiply and Integrate Term-by-Term**

We now multiply the two series and integrate term-by-term:

$$
\int_0^1 \mathbf{L}_0(2\sqrt{x}) \, \mathbf{E}(\sqrt{1 - x}) \, dx = \int_0^1 \left( \sqrt{x} \sum_{k=0}^{\infty} \frac{x^k}{\Gamma(k + 3/2)^2} \right) \left( \frac{\pi}{2} \sum_{n=0}^{\infty} \frac{(-1/2)_n (1/2)_n}{(1)_n n!} (1 - x)^n \right) dx.
$$

Interchanging summation and integration (justified by uniform convergence), we get:

$$
\frac{\pi}{2} \sum_{k=0}^{\infty} \sum_{n=0}^{\infty} \frac{(-1/2)_n (1/2)_n}{(1)_n n!} \cdot \frac{1}{\Gamma(k + 3/2)^2} \int_0^1 x^{k + 1/2} (1 - x)^n dx.
$$

The integral is a Beta function:

$$
\int_0^1 x^{k + 1/2} (1 - x)^n dx = B(k + 3/2, n + 1) = \frac{\Gamma(k + 3/2) \Gamma(n + 1)}{\Gamma(k + n + 5/2)}.
$$

Substituting this back, we obtain:

$$
\frac{\pi}{2} \sum_{k=0}^{\infty} \sum_{n=0}^{\infty} \frac{(-1/2)_n (1/2)_n}{(1)_n n!} \cdot \frac{\Gamma(k + 3/2) \Gamma(n + 1)}{\Gamma(k + 3/2)^2 \Gamma(k + n + 5/2)}.
$$

Simplifying:

$$
\frac{\pi}{2} \sum_{k=0}^{\infty} \sum_{n=0}^{\infty} \frac{(-1/2)_n (1/2)_n}{(1)_n} \cdot \frac{1}{\Gamma(k + 3/2) \Gamma(k + n +