We wish to evaluate

  I = ∫₀^(π/4) ln(cot x – 1) dx.

Step 1. Rewrite the integrand.

Recall that cot x = cos x/sin x, so
  cot x – 1 = (cos x – sin x)/sin x.
Taking the logarithm yields
  ln(cot x – 1) = ln(cos x – sin x) – ln(sin x).

Thus,
  I = ∫₀^(π/4) [ln(cos x – sin x) – ln(sin x)] dx.

Step 2. Simplify ln(cos x – sin x).

Notice that
  cos x – sin x = √2 cos(x + π/4),
since
  cos(x + π/4) = (cos x cos(π/4) – sin x sin(π/4)) = (cos x – sin x)/√2.
Thus,
  ln(cos x – sin x) = ln(√2 cos(x + π/4)) = ln(√2) + ln(cos(x + π/4)).

Now the integral becomes
  I = ∫₀^(π/4) [ln(√2) + ln(cos(x+π/4)) – ln(sin x)] dx
    = (ln √2) ∫₀^(π/4) dx + ∫₀^(π/4) ln(cos(x+π/4)) dx – ∫₀^(π/4) ln(sin x) dx.

Since ∫₀^(π/4) dx = π/4, the first term is (π/4) ln(√2).

Step 3. Change the variable in the cosine integral.

Let u = x + π/4, so that du = dx. When x = 0, u = π/4; when x = π/4, u = π/2. Thus,

  ∫₀^(π/4) ln(cos(x+π/4)) dx = ∫_(π/4)^(π/2) ln(cos u) du.

Now the integral I becomes
  I = (π/4) ln(√2) + ∫_(π/4)^(π/2) ln(cos u) du – ∫₀^(π/4) ln(sin x) dx.

Step 4. Relate the two integrals.

Perform a substitution in the cosine integral: Let v = π/2 – u so that dv = –du. When u = π/4, then v = π/4; when u = π/2, v = 0. Therefore,
  ∫_(π/4)^(π/2) ln(cos u) du = ∫_(π/4)^(0) ln(cos(π/2 – v)) (–dv)
    = ∫₀^(π/4) ln(sin v) dv.
That is, this integral equals ∫₀^(π/4) ln(sin x) dx (renaming the variable).

Thus, we see that
  ∫_(π/4)^(π/2) ln(cos u) du – ∫₀^(π/4) ln(sin x) dx = 0.

Step 5. Conclude.

Therefore, the entire integral reduces to
  I = (π/4) ln(√2).
Since ln(√2) = ½ ln 2, we have
  I = (π/4) × (½ ln 2) = (π/8) ln 2.

Step 6. Numerical approximation.

Using π ≈ 3.1415926536 and ln 2 ≈ 0.6931471806, we compute:
  I ≈ (3.1415926536/8) × 0.6931471806 ≈ 0.3926990817 × 0.6931471806 ≈ 0.2721982613.

Thus, the final answer is:

{"answer": "\\frac{\\pi}{8}\\ln2", "numerical_answer": "0.2721982613"}