
To solve the definite integral \(\int_0^{\frac{\pi}{2}}\frac{\cos^2x(1+\cos x)}{(1+\cos x+\sin x)^2}\mathrm{d}x\), we proceed as follows:

### Step 1: Substitution for Symmetry
Consider the substitution \(t = \frac{\pi}{2} - x\). This transforms the integral into:
\[
I = \int_0^{\frac{\pi}{2}} \frac{\sin^2 t (1 + \sin t)}{(1 + \cos t + \sin t)^2} \mathrm{d}t
\]
Since \(t\) is a dummy variable, we rewrite it as \(x\), so:
\[
I = \int_0^{\frac{\pi}{2}} \frac{\sin^2 x (1 + \sin x)}{(1 + \cos x + \sin x)^2} \mathrm{d}x
\]

### Step 2: Adding the Original and Substituted Integrals
Add the original integral \(I\) and the substituted integral \(I\):
\[
2I = \int_0^{\frac{\pi}{2}} \frac{\cos^2 x (1 + \cos x) + \sin^2 x (1 + \sin x)}{(1 + \cos x + \sin x)^2} \mathrm{d}x
\]

### Step 3: Simplifying the Numerator
The numerator simplifies using \(\cos^2 x + \sin^2 x = 1\) and factoring \(\cos^3 x + \sin^3 x\):
\[
\cos^2 x (1 + \cos x) + \sin^2 x (1 + \sin x) = 1 + \cos^3 x + \sin^3 x = 1 + (\cos x + \sin x)(1 - \cos x \sin x)
\]

### Step 4: Further Simplification
Let \(S = \cos x + \sin x\). Then \(\cos x \sin x = \frac{S^2 - 1}{2}\). Substituting these into the numerator:
\[
1 + S - S \cdot \frac{S^2 - 1}{2} = \frac{2 + 3S - S^3}{2}
\]
Factoring \(S^3 - 3S - 2 = (S + 1)^2(S - 2)\), we rewrite the numerator as \(\frac{(S + 1)^2(2 - S)}{2}\). The denominator is \((1 + S)^2\), so they cancel, leaving \(\frac{2 - S}{2}\).

### Step 5: Evaluating the Integral
The integral simplifies to:
\[
2I = \frac{1}{2} \int_0^{\frac{\pi}{2}} (2 - (\cos x + \sin x)) \mathrm{d}x
\]
Evaluating the integral:
\[
\int_0^{\frac{\pi}{2}} 2 \mathrm{d}x = \pi, \quad \int_0^{\frac{\pi}{2}} \cos x \mathrm{d}x = 1, \quad \int_0^{\frac{\pi}{2}} \sin x \mathrm{d}x = 1
\]
Thus:
\[
2I = \frac{1}{2}(\pi - 1 - 1) = \frac{\pi - 2}{2}
\]
Finally, \(I = \frac{\pi - 2}{4}\).

### Numerical Approximation
The numerical value of \(\frac{\pi - 2}{4}\) is approximately \(0.2853981634\).

{"answer": "\\frac{\\pi - 2}{4}", "numerical_answer": "0.2853981634"}