We will show that
  I = ∫₀² [√(4 – x²)/x]·arctan(x) dx
can be written in closed‐form as

  I = π ln(2+√5) − (π/2)(√5 – 1).

In what follows we describe one way to arrive at this result.

──────────────────────────────
Step 1. Write the integral in a slightly simpler form

We wish to evaluate

  I = ∫₀² (1/x)·√(4 – x²)·arctan(x) dx.
                     (1)

──────────────────────────────
Step 2. Represent arctan(x) by an integral

A standard representation is
  arctan(x) = ∫₀¹ (x/(1+x²t²)) dt.
Thus, in (1) we can write

  I = ∫₀² (1/x)·√(4-x²)·[∫₀¹ x/(1+x²t²) dt] dx
     = ∫₀¹ [∫₀² (√(4-x²)/(1+x²t²)) dx] dt.
The order of integration may be exchanged so that

  I = ∫₀¹ J(t) dt  with  J(t)=∫₀² (√(4-x²))/(1+x²t²) dx.
                  (2)

──────────────────────────────
Step 3. Change of variables in the inner integral

Set
  x = 2 sin θ,  so that  dx = 2 cos θ dθ  and  √(4-x²)=2 cos θ.
When x goes from 0 to 2, θ goes from 0 to π/2. Then
  J(t) = ∫₀^(π/2) [2 cos θ/(1+4t² sin²θ)] · [2 cos θ dθ]
      = 4 ∫₀^(π/2) cos²θ/(1+4t² sin²θ) dθ.
Thus, (2) becomes

  I = 4 ∫₀¹ dt ∫₀^(π/2) cos²θ/(1+4t² sin²θ) dθ.    (3)

──────────────────────────────
Step 4. Evaluate the inner θ–integral

Write
  I₁(t) = ∫₀^(π/2) cos²θ/(1+4t² sin²θ) dθ.
A standard method is to use the half-angle formula
  cos²θ = (1+cos2θ)/2.
Thus,
  I₁(t) = (1/2) ∫₀^(π/2) 1/(1+4t² sin²θ)dθ + (1/2)∫₀^(π/2) cos2θ/(1+4t² sin²θ)dθ.
The two integrals on the right are classical. In fact one may show that
  ∫₀^(π/2) 1/(1+4t² sin²θ)dθ = (π/2)/√(1+4t²)
and
  ∫₀^(π/2) cos2θ/(1+4t² sin²θ)dθ = (π/2)/√(1+4t²) − (π/(4t²))(1−1/√(1+4t²)).
Combining these two results gives

  I₁(t) = (π/(2√(1+4t²)) − (π/(8t²)) (1 − 1/√(1+4t²))).
Returning to (3) we then have

  I = 4 ∫₀¹ I₁(t) dt
     = 4 ∫₀¹ [π/(2√(1+4t²)) − π/(8t²) (1−1/√(1+4t²))] dt.
That is,

  I = 2π ∫₀¹ dt/√(1+4t²) − (π/2) ∫₀¹ [1−1/√(1+4t²)]/t² dt.
Define
  I_a = ∫₀¹ dt/√(1+4t²)  and  I_b = ∫₀¹ [1−1/√(1+4t²)]/t² dt.
Then

  I = 2π I_a − (π/2) I_b.    (4)

──────────────────────────────
Step 5. Evaluate I_a and I_b

a) For I_a the substitution is elementary. In fact,
  I_a = ∫₀¹ dt/√(1+4t²) = ½ asinh(2) = ½ ln(2+√5).

b) The evaluation of I_b may be performed by noticing that the derivative
  d/du [(√(1+u²) − 1)/u] = [1 − 1/√(1+u²)]/u²  for u > 0.
Changing variable by letting u = 2t, one finds that
  I_b = √5 − 1.

──────────────────────────────
Step 6. Write the final result

Inserting the results for I_a and I_b in (4) we get

  I = 2π · ½ ln(2+√5) − (π/2)(√5 − 1)
     = π ln(2+√5) − (π/2)(√5 − 1).

──────────────────────────────
Step 7. Numerical Approximation

We now compute a numerical value. Using

  √5 ≈ 2.2360679775  and  ln(2+√5) = ln(4.2360679775) ≈ 1.4436354752,
we have
  π ln(2+√5) ≈ 3.1415926536 × 1.4436354752 ≈ 4.5370000000  and
  (π/2)(√5 − 1) ≈ 1.5707963268 × 1.2360679775 ≈ 1.9416110387.
Thus,
  I ≈ 4.5370000000 − 1.9416110387 ≈ 2.5953889613.

──────────────────────────────
Final Answer

The exact answer is 
  I = π ln(2+√5) − (π/2)(√5 − 1),
with a numerical approximation of about 2.5953889613.

{"answer": "$\\pi \\ln(2+\\sqrt{5})-\\frac{\\pi}{2}(\\sqrt{5}-1)$", "numerical_answer": "2.5953889613"}