<think>
Okay, let's tackle this integral step by step. The integral given is from 0 to 1.0 of x times the natural logarithm of (1.0 + sqrt(1.0² - x²))/x, multiplied by the differential D(0.5x) dx. Hmm, first, I need to make sure I understand the notation here. The D(0.5x) part might be a bit confusing. Wait, in some contexts, D could denote the differential operator, but here it's probably a notation for the derivative. So D(0.5x) would be the derivative of 0.5x with respect to x. Let me check that. The derivative of 0.5x with respect to x is just 0.5. So maybe the integral is actually ∫₀¹ x ln[(1 + √(1 - x²))/x] * 0.5 dx. That makes sense. So the D(0.5x) is the derivative, which is 0.5 dx. So the integral simplifies to 0.5 ∫₀¹ x ln[(1 + √(1 - x²))/x] dx.

Alright, let's rewrite the integral for clarity: 0.5 ∫₀¹ x ln[(1 + √(1 - x²))/x] dx. Now, the integrand is x multiplied by a logarithm of a somewhat complicated expression. Let me see if I can simplify the logarithm first. The argument inside the log is (1 + sqrt(1 - x²))/x. Let's denote that as (1 + sqrt(1 - x²))/x. Maybe there's a substitution that can simplify this expression.

Let me consider a substitution to handle the square root. The sqrt(1 - x²) suggests a trigonometric substitution, like x = sinθ, since 1 - sin²θ = cos²θ. Let's try that. Let x = sinθ, so dx = cosθ dθ. Then, when x = 0, θ = 0, and when x = 1, θ = π/2. Let's substitute these into the integral.

First, sqrt(1 - x²) becomes sqrt(1 - sin²θ) = cosθ. Then, the argument of the log becomes (1 + cosθ)/sinθ. So the integral becomes 0.5 ∫₀^{π/2} sinθ * ln[(1 + cosθ)/sinθ] * cosθ dθ. Wait, because x is sinθ, so x in the original integrand is sinθ, and dx is cosθ dθ. So the original integrand x ln(...) dx becomes sinθ * ln[(1 + cosθ)/sinθ] * cosθ dθ. Then multiplied by the 0.5 factor. So combining terms, the integral is 0.5 ∫₀^{π/2} sinθ * cosθ * ln[(1 + cosθ)/sinθ] dθ.

Hmm, that's a bit complicated. Let's simplify the logarithm term. The expression (1 + cosθ)/sinθ can be rewritten using trigonometric identities. Recall that 1 + cosθ = 2 cos²(θ/2), and sinθ = 2 sin(θ/2) cos(θ/2). So substituting these in, we get (2 cos²(θ/2)) / (2 sin(θ/2) cos(θ/2)) ) = cos(θ/2)/sin(θ/2) = cot(θ/2). Therefore, ln[(1 + cosθ)/sinθ] = ln(cot(θ/2)) = ln(1/tan(θ/2)) = -ln(tan(θ/2)). So the integral becomes 0.5 ∫₀^{π/2} sinθ cosθ (-ln(tan(θ/2))) dθ. Let's write that as -0.5 ∫₀^{π/2} sinθ cosθ ln(tan(θ/2)) dθ.

Alternatively, maybe there's another substitution. Let me think. Alternatively, perhaps integrating by parts. Let's consider integrating by parts. Let u = ln[(1 + sqrt(1 - x²))/x], dv = x dx. Wait, but in the original integral, it's 0.5 x ln(...) dx, so maybe set u = ln[(1 + sqrt(1 - x²))/x], dv = 0.5 x dx. Then du would be the derivative of the log term times dx, and v would be the integral of 0.5 x dx, which is 0.25 x². Let's try that.

But before proceeding, let me compute du. Let me compute the derivative of ln[(1 + sqrt(1 - x²))/x]. Let me denote the argument as A = (1 + sqrt(1 - x²))/x. Then ln A, so derivative is (A')/A. Let's compute A':

A = (1 + sqrt(1 - x²))/x. Let's differentiate numerator and denominator. Let me write A = [1 + (1 - x²)^{1/2}]/x. Then A' = [ derivative of numerator * x - numerator * derivative of denominator ] / x².

Derivative of numerator: d/dx [1 + (1 - x²)^{1/2}] = 0 + (1/2)(1 - x²)^{-1/2}*(-2x) = -x / sqrt(1 - x²).

Derivative of denominator (x) is 1. So A' = [ (-x / sqrt(1 - x²)) * x - (1 + sqrt(1 - x²)) * 1 ] / x².

Simplify numerator of A':

First term: (-x²)/sqrt(1 - x²)

Second term: - (1 + sqrt(1 - x²))

So combining: [ -x² / sqrt(1 - x²) - 1 - sqrt(1 - x²) ] / x²

Hmm, this seems messy. Maybe there's a better substitution. Let's go back to the trigonometric substitution. So we had the integral as -0.5 ∫₀^{π/2} sinθ cosθ ln(tan(θ/2)) dθ. Let's see if we can manipulate this.

Alternatively, perhaps changing variables. Let me set t = θ/2, so θ = 2t, dθ = 2dt. Then the limits when θ=0, t=0; θ=π/2, t=π/4. Then the integral becomes -0.5 ∫₀^{π/4} sin(2t) cos(2t) ln(tan t) * 2 dt. The 2 comes from dθ = 2dt. So the constants: -0.5 * 2 = -1. So integral is -1 * ∫₀^{π/4} sin(2t) cos(2t) ln(tan t) dt.

But sin(2t) cos(2t) can be simplified. Recall that sin(2t) cos(2t) = (1/2) sin(4t). So substituting that in, the integral becomes -1 * ∫₀^{π/4} (1/2) sin(4t) ln(tan t) dt = - (1/2) ∫₀^{π/4} sin(4t) ln(tan t) dt.

Hmm, this seems more complicated. Maybe integrating by parts here. Let me set u = ln(tan t), dv = sin(4t) dt. Then du = [1/tan t * sec² t] dt = [cot t * sec² t] dt. Wait, derivative of ln(tan t) is (sec² t)/tan t = (1/cos² t) * (cos t / sin t) ) = 1/(sin t cos t). So du = 1/(sin t cos t) dt. And v is the integral of sin(4t) dt, which is - (1/4) cos(4t).

So integrating by parts: uv|₀^{π/4} - ∫₀^{π/4} v du. So:

- (1/2) [ uv|₀^{π/4} - ∫ v du ]

First, compute uv at π/4 and 0. At t=π/4, ln(tan π/4) = ln(1) = 0. So uv at π/4 is 0 * (-1/4 cos(4*(π/4))) = 0. At t=0, tan t approaches 0, so ln(tan t) approaches -infinity, but multiplied by v which is -1/4 cos(0) = -1/4. However, the limit as t approaches 0 from the right of ln(tan t) * (-1/4 cos(4t)) would be (-1/4)(1) * (-infty), which is +infty. But this suggests that the integral might diverge, but the original integral is from 0 to 1, which is finite. So perhaps there's a mistake in substitution steps.

Wait, maybe the substitution steps have an error. Let me check again. The original integral is from 0 to 1.0. When we did the substitution x = sinθ, θ goes from 0 to π/2. Then, when we changed variables to t = θ/2, t goes from 0 to π/4. So the integral in terms of t is from 0 to π/4. But when t approaches 0, tan t approaches 0, so ln(tan t) approaches -infty. However, the original integrand at x approaching 0: x ln[(1 + sqrt(1 - x²))/x]. Let's check the behavior as x approaches 0. The term inside the log is (1 + sqrt(1 - x²))/x ≈ (1 + 1 - x²/2)/x ≈ (2 - x²/2)/x ≈ 2/x as x approaches 0. So ln(2/x) = ln 2 - ln x. So the integrand near 0 is x*(ln 2 - ln x). As x approaches 0, x ln x approaches 0 (since x ln x tends to 0), so the integrand approaches x ln 2, which is 0. So the original integral is convergent. Therefore, the substitution steps must be correct, and the apparent divergence in the intermediate steps must cancel out. So perhaps the boundary term in the integration by parts is actually finite.

Wait, when t approaches 0, ln(tan t) approaches -infty, but v is -1/4 cos(4t). At t=0, cos(0) = 1, so v is -1/4. So uv at t approaching 0 is (-1/4) * (-infty) = +infty. But the other term at t=π/4 is 0. So uv evaluated from 0 to π/4 would be 0 - (-infty), which is +infty. But this contradicts the original integral being finite. Therefore, there's a mistake in the integration by parts approach here. Maybe integrating by parts isn't the right way, or perhaps I made a miscalculation.

Alternatively, perhaps the substitution is not the best approach. Let me try another substitution. Let's go back to the original integral: 0.5 ∫₀¹ x ln[(1 + sqrt(1 - x²))/x] dx. Let me make a substitution to simplify the logarithm. Let me set y = sqrt(1 - x²). Then, y = sqrt(1 - x²), so y² = 1 - x², so x² = 1 - y², and x dx = - y dy. Let's see. Differentiating both sides: 2x dx = -2y dy, so x dx = - y dy. So when x=0, y=1, and when x=1, y=0. So the limits would invert. Let's substitute:

The integral becomes 0.5 ∫_{y=1}^{y=0} x ln[(1 + y)/x] * (- y dy / x). Wait, x dx = - y dy, so dx = - y dy / x. But in the original integral, we have x ln(...) dx. So substituting, x ln(...) dx becomes x ln[(1 + y)/x] * (- y dy / x) = - y ln[(1 + y)/x] dy. But x is sqrt(1 - y²). Wait, because y = sqrt(1 - x²), so x = sqrt(1 - y²). So substituting x in terms of y, we have:

- y ln[(1 + y)/sqrt(1 - y²)] dy. The limits are from y=1 to y=0, but with the negative sign, it becomes ∫₀¹ y ln[(1 + y)/sqrt(1 - y²)] dy. So the integral is 0.5 times that, right? Wait, original substitution: 0.5 ∫₀¹ x ln(...) dx becomes 0.5 * ∫₀¹ y ln[(1 + y)/sqrt(1 - y²)] dy. Wait, let me check again.

Original integral: 0.5 ∫₀¹ x ln[(1 + sqrt(1 - x²))/x] dx.

Substitution: y = sqrt(1 - x²), so x = sqrt(1 - y²), dx = - y dy / x. Then, x dx = - y dy. Wait, maybe I need to re-express the integral correctly.

Wait, when we substitute y = sqrt(1 - x²), then x goes from 0 to 1, y goes from 1 to 0. So the integral becomes:

0.5 ∫_{1}^{0} x ln[(1 + y)/x] * ( - y / x ) dy. Because dx = - y / x dy. So the x in the numerator and denominator cancels, and the negative sign flips the limits:

0.5 ∫₀¹ y ln[(1 + y)/x] dy. But x is sqrt(1 - y²), so substituting that in:

0.5 ∫₀¹ y ln[(1 + y)/sqrt(1 - y²)] dy.

Simplify the logarithm: ln(1 + y) - (1/2) ln(1 - y²). So the integral becomes 0.5 ∫₀¹ y [ln(1 + y) - (1/2) ln(1 - y²)] dy.

Which can be split into two integrals:

0.5 [ ∫₀¹ y ln(1 + y) dy - (1/2) ∫₀¹ y ln(1 - y²) dy ].

Let me compute these two integrals separately.

First integral: I1 = ∫₀¹ y ln(1 + y) dy.

Second integral: I2 = ∫₀¹ y ln(1 - y²) dy.

Compute I1: Integration by parts. Let u = ln(1 + y), dv = y dy. Then du = 1/(1 + y) dy, v = (1/2)y².

So I1 = uv|₀¹ - ∫₀¹ v du = [ (1/2)y² ln(1 + y) ]₀¹ - ∫₀¹ (1/2)y² * 1/(1 + y) dy.

Evaluate the first term at 1: (1/2)(1)² ln(2) - (1/2)(0)² ln(1) = (1/2) ln 2.

At 0, the term is 0. So the first part is (1/2) ln 2.

Now compute the remaining integral: ∫₀¹ (1/2)y² / (1 + y) dy.

Factor out 1/2: (1/2) ∫₀¹ y²/(1 + y) dy.

Simplify the integrand: y²/(1 + y) = (y² - 1 + 1)/(1 + y) = (y - 1)(y + 1)/(1 + y) + 1/(1 + y) = (y - 1) + 1/(1 + y).

Wait, that's a standard technique. Let me do polynomial division. Divide y² by (y + 1):

y² ÷ (y + 1) = y - 1 with a remainder of 1. So y² = (y + 1)(y - 1) + 1. Therefore, y²/(y + 1) = y - 1 + 1/(y + 1).

So the integral becomes (1/2) ∫₀¹ [y - 1 + 1/(y + 1)] dy = (1/2)[ ∫₀¹ y dy - ∫₀¹ 1 dy + ∫₀¹ 1/(y + 1) dy ].

Compute each part:

∫₀¹ y dy = (1/2)y² |₀¹ = 1/2.

∫₀¹ 1 dy = 1.

∫₀¹ 1/(y + 1) dy = ln|y + 1| |₀¹ = ln 2 - ln 1 = ln 2.

So combining these:

(1/2)[ (1/2 - 1 + ln 2) ] = (1/2)( -1/2 + ln 2 ) = -1/4 + (1/2) ln 2.

Therefore, I1 = (1/2) ln 2 - ( -1/4 + (1/2) ln 2 ) = (1/2) ln 2 + 1/4 - (1/2) ln 2 = 1/4.

Wait, wait, no. Wait, the original I1 was [ (1/2) ln 2 ] minus the integral which was computed as -1/4 + (1/2) ln 2. So:

I1 = (1/2) ln 2 - [ -1/4 + (1/2) ln 2 ] = (1/2) ln 2 + 1/4 - (1/2) ln 2 = 1/4.

So I1 = 1/4.

Now compute I2 = ∫₀¹ y ln(1 - y²) dy.

Again, use substitution. Let u = 1 - y², then du = -2y dy. So y dy = - du/2. When y=0, u=1; y=1, u=0. So I2 = ∫_{u=1}^{u=0} ln(u) * (-du/2) = (1/2) ∫₀¹ ln u du.

The integral of ln u du is u ln u - u. So evaluated from 0 to 1:

At u=1: 1*0 -1 = -1.

At u=0: the limit as u approaches 0+ of u ln u - u is 0 - 0 = 0.

So ∫₀¹ ln u du = -1. Therefore, I2 = (1/2)(-1) = -1/2.

So going back to the original expression:

0.5 [ I1 - (1/2) I2 ] = 0.5 [ 1/4 - (1/2)(-1/2) ] = 0.5 [ 1/4 + 1/4 ] = 0.5 [ 1/2 ] = 1/4.

Wait, let me check that again. The original split was:

0.5 [ I1 - (1/2) I2 ].

I1 is 1/4, I2 is -1/2. So substituting:

0.5 [ 1/4 - (1/2)(-1/2) ] = 0.5 [ 1/4 + 1/4 ] = 0.5 [ 1/2 ] = 1/4.

So the value of the original integral is 1/4.

Wait, the exact answer is 1/4? Let me verify this with a numerical approximation. Let's compute the integral numerically to check.

The integral is 0.5 ∫₀¹ x ln[(1 + sqrt(1 - x²))/x] dx. Let's approximate this numerically. Let's take x from 0 to 1, and compute the integrand at several points.

Alternatively, since we have the exact answer as 1/4, which is 0.25. Let's check with a simple approximation. For example, at x=1, the integrand is 0.5*1*ln[(1 + 0)/1] = 0.5*1*ln(1) = 0. But the integral from 0 to 1 of a function that starts at 0 (since as x approaches 0, x ln(2/x) ~ x ln(1/x) which tends to 0) and ends at 0, peaking somewhere in between. The exact answer is 0.25. Let's compute a rough numerical estimate.

Alternatively, use substitution. Let me compute the integral numerically using substitution. Let x = sinθ, then the integral becomes 0.5 ∫₀^{π/2} sinθ cosθ ln[(1 + cosθ)/sinθ] dθ. Let's compute this integral numerically. Let's approximate θ from 0 to π/2. Let's take θ = 0 to π/2 in steps. Alternatively, use a calculator or approximate using known integrals.

Alternatively, since we derived the exact answer as 1/4, which is 0.25, and the numerical approximation should be around 0.25. Let's check with x=0.5. The integrand is 0.5*0.5*ln[(1 + sqrt(1 - 0.25))/0.5] = 0.25*ln[(1 + sqrt(0.75))/0.5]. sqrt(0.75) ≈ 0.8660, so 1 + 0.8660 ≈ 1.8660. Divide by 0.5: 3.732. ln(3.732) ≈ 1.317. So the integrand at x=0.5 is 0.25*1.317 ≈ 0.329. The integral from 0 to 1 would be the area under the curve. Since the function starts at 0, rises to a peak, and goes back to 0, the area might be around 0.25. Let's take another point, x=0.7071 (sqrt(0.5)). Then sqrt(1 - x²) = sqrt(1 - 0.5) = sqrt(0.5) ≈ 0.7071. So the argument of the log is (1 + 0.7071)/0.7071 ≈ 1.7071/0.7071 ≈ 2.4142. ln(2.4142) ≈ 0.88. The integrand is 0.5*0.7071*0.88 ≈ 0.5*0.7071*0.88 ≈ 0.5*0.622 ≈ 0.311. So the integrand is positive throughout, and integrating to 0.25 seems plausible.

Therefore, the exact answer is 1/4, and the numerical approximation is 0.25. So the JSON output should be {"answer": "\frac{1}{4}", "numerical_answer": "0.2500000000"}.
</think>

{"answer": "\\frac{1}{4}", "numerical_answer": "0.2500000000"}