To compute the definite integral \(\int_{-1}^1 \frac{\cos x}{1 + e^{-\frac{1}{x}}} \, dx\), we will follow these steps:

### Step 1: Simplify the Integrand
First, observe the integrand \(\frac{\cos x}{1 + e^{-\frac{1}{x}}}\). For \(x \in (0, 1]\), \(e^{-\frac{1}{x}}\) is very small (since \(\frac{1}{x}\) is large and positive), so \(1 + e^{-\frac{1}{x}} \approx 1\). For \(x \in [-1, 0)\), \(e^{-\frac{1}{x}}\) is very large (since \(\frac{1}{x}\) is negative), so \(1 + e^{-\frac{1}{x}} \approx e^{-\frac{1}{x}}\), and the integrand becomes \(\frac{\cos x}{e^{-\frac{1}{x}}} = \cos x \cdot e^{\frac{1}{x}}\).

However, the integrand is not defined at \(x = 0\) because \(e^{-\frac{1}{x}}\) is not defined there. But we can consider the integral as a limit approaching 0 from both sides.

### Step 2: Symmetry and Substitution
Let \(I = \int_{-1}^1 \frac{\cos x}{1 + e^{-\frac{1}{x}}} \, dx\). Split the integral at \(x = 0\):
\[
I = \int_{-1}^0 \frac{\cos x}{1 + e^{-\frac{1}{x}}} \, dx + \int_{0}^1 \frac{\cos x}{1 + e^{-\frac{1}{x}}} \, dx.
\]

For the first integral, make the substitution \(x = -t\), \(dx = -dt\):
\[
\int_{-1}^0 \frac{\cos x}{1 + e^{-\frac{1}{x}}} \, dx = \int_{1}^0 \frac{\cos(-t)}{1 + e^{\frac{1}{t}}} (-dt) = \int_{0}^1 \frac{\cos t}{1 + e^{\frac{1}{t}}} \, dt.
\]

Now, observe that:
\[
\frac{1}{1 + e^{\frac{1}{t}}} = 1 - \frac{1}{1 + e^{-\frac{1}{t}}}.
\]

Thus, the integral becomes:
\[
I = \int_{0}^1 \cos t \left(1 - \frac{1}{1 + e^{-\frac{1}{t}}}\right) dt + \int_{0}^1 \frac{\cos t}{1 + e^{-\frac{1}{t}}} \, dt = \int_{0}^1 \cos t \, dt.
\]

### Step 3: Compute the Simplified Integral
The integral simplifies to:
\[
I = \int_{0}^1 \cos t \, dt = \sin t \Big|_{0}^1 = \sin 1 - \sin 0 = \sin 1.
\]

### Step 4: Numerical Approximation
The exact answer is \(\sin 1\). Numerically, this is approximately:
\[
\sin 1 \approx 0.8414709848.
\]

### Final Answer
```json
{"answer": "\\sin(1)", "numerical_answer": "0.8414709848"}
```