<think>
Okay, let's tackle this integral step by step. The integral given is ∫₀¹ (1/x) * ln[(1+√x)/(1-√x)] * K(√(1 - x)) dx. Hmm, that looks a bit complicated, but maybe we can simplify it with some substitutions or known integral formulas.

First, let me recall that K(k) is the complete elliptic integral of the first kind, defined as K(k) = ∫₀^(π/2) dθ / √(1 - k² sin²θ). So here, the argument of K is √(1 - x), which means k = √(1 - x). Maybe changing variables to make the argument of K simpler could help.

Let me consider a substitution. Let’s set t = √x. Then x = t², so dx = 2t dt. When x goes from 0 to 1, t goes from 0 to 1. Let's rewrite the integral in terms of t:

Integral becomes ∫₀¹ (1/t²) * ln[(1 + t)/(1 - t)] * K(√(1 - t²)) * 2t dt. Simplifying, the 1/t² and 2t give 2/t. So:

2 ∫₀¹ [ln((1 + t)/(1 - t)) / t] * K(√(1 - t²)) dt.

Hmm, the term ln[(1 + t)/(1 - t)] / t is familiar. Let me recall that ln[(1 + t)/(1 - t)] is 2 artanh(t), so maybe expanding this as a series could help. The Maclaurin series for artanh(t) is t + t³/3 + t⁵/5 + ... for |t| < 1. So ln[(1 + t)/(1 - t)] = 2 artanh(t) = 2(t + t³/3 + t⁵/5 + ...). Therefore, dividing by t gives 2(1 + t²/3 + t⁴/5 + ...). So the integrand becomes 2 * [2(1 + t²/3 + t⁴/5 + ...)] * K(√(1 - t²)) dt. Wait, but that's 4 times the sum. Wait, no, the original integral after substitution is 2 ∫ [ln(...)/t] * K(...) dt, and ln(...)/t is 2 artanh(t)/t, which is 2*(1 + t²/3 + t⁴/5 + ...). So the integral becomes 2 * 2 ∫₀¹ [1 + t²/3 + t⁴/5 + ...] * K(√(1 - t²)) dt. So 4 times the sum over n of (1/(2n + 1)) ∫₀¹ t^{2n} K(√(1 - t²)) dt. Hmm, but integrating term by term might be complicated. Maybe there's a better substitution.

Alternatively, let's consider another substitution. Let’s set u = √(1 - t²), where t is from 0 to 1. Wait, if t is from 0 to 1, then u goes from 1 to 0. But maybe that's not helpful. Alternatively, perhaps express K(√(1 - t²)) in terms of another elliptic integral. Wait, there's a relation between K(k) and K'(k) = K(√(1 - k²}), which is the complementary modulus. But here, the argument is already √(1 - t²), so maybe K(√(1 - t²)) is K'(t). Wait, K'(k) is usually defined as K(√(1 - k²}), so if we let k = t, then K'(t) = K(√(1 - t²)). So the integral becomes 2 ∫₀¹ [ln((1 + t)/(1 - t))/t] * K'(t) dt. Hmm, that might be a useful notation.

So the integral is 2 ∫₀¹ [2 artanh(t)/t] * K'(t) dt. Which is 4 ∫₀¹ [artanh(t)/t] * K'(t) dt. But I'm not sure if that helps directly. Maybe integrating by parts? Let’s consider integrating K'(t) and differentiating the other part. Let’s set u = artanh(t)/t, dv = K'(t) dt. Then du would be [ (1/(1 - t²)) * t - artanh(t) ] / t² dt. Hmm, that seems messy. Alternatively, maybe switch the order of integration or use some integral representation of K'.

Alternatively, perhaps use a substitution to relate this integral to known results involving elliptic integrals and logarithmic functions. Let me check some standard integrals. For example, integrals involving K(k) and logarithmic terms. Alternatively, maybe express the logarithm as an integral. For example, ln[(1 + t)/(1 - t)] = 2 ∫₀^t 1/(1 - s²) ds. So maybe we can write the original integral as 2 ∫₀¹ [2 ∫₀^t 1/(1 - s²) ds / t] * K'(t) dt. Then switching the order of integration. The region is 0 ≤ s ≤ t ≤1. So changing the order, s goes from 0 to1, and t goes from s to1. So the integral becomes 4 ∫₀¹ [1/(1 - s²)] ∫_{t=s}^1 [K'(t)/t] dt ds. Hmm, not sure if that helps. Let me compute the inner integral ∫_{s}^1 K'(t)/t dt. If we can find an antiderivative for K'(t)/t, that might be useful, but I don't recall such a formula.

Alternatively, perhaps use the series expansion of K'(t). The complete elliptic integral of the first kind can be expressed as a series: K(k) = (π/2) Σ_{n=0}^∞ [( (2n)! ) / (2^{2n} (n!)^2 )]^2 k^{2n}. So K'(k) = K(√(1 - k²}) = (π/2) Σ_{n=0}^∞ [( (2n)! ) / (2^{2n} (n!)^2 )]^2 (1 - k²)^n. But substituting that into the integral might lead to a complicated expression. Alternatively, maybe use hypergeometric functions, but this seems too vague.

Wait, perhaps there's a known integral formula that combines K(k) and logarithmic functions. Let me think. Alternatively, consider using substitution to relate the integral to derivatives of elliptic integrals. For example, integrating by parts with K'(t). Let me try integrating by parts. Let’s set u = ln[(1 + t)/(1 - t)] / t, dv = K'(t) dt. Then du would be derivative of that, and v = ∫ K'(t) dt. But I don't know the integral of K'(t) off the top of my head. Wait, but K'(t) = K(√(1 - t²}), and integrating that with respect to t might not be straightforward. Alternatively, maybe use differentiation under the integral sign. Let’s consider if the integral can be expressed as a derivative of some known integral.

Alternatively, let's consider changing variables to x = t². Wait, but we already did that. Maybe another substitution. Let’s set y = √(1 - t²). Then t = √(1 - y²), dt = - y / √(1 - y²) dy. Hmm, but when t goes from 0 to1, y goes from1 to0. So the integral becomes 2 ∫₁⁰ [ln((1 + √(1 - y²))/(1 - √(1 - y²))) / √(1 - y²))] * K(y) * (- y / √(1 - y²)) dy. The negative sign flips the limits back to 0 to1. So:

2 ∫₀¹ [ln((1 + √(1 - y²))/(1 - √(1 - y²))) / √(1 - y²)] * K(y) * (y / √(1 - y²)) dy.

Simplify the terms: 2 ∫₀¹ y / (1 - y²) * ln[(1 + √(1 - y²))/(1 - √(1 - y²))] * K(y) dy.

Hmm, this seems more complicated. The logarithm term now involves √(1 - y²). Let me rationalize the argument of the logarithm. Let’s set z = √(1 - y²), so 1 - z² = y². Then the argument becomes (1 + z)/(1 - z). Let’s compute that:

(1 + z)/(1 - z) = [1 + √(1 - y²)]/[1 - √(1 - y²)]. Multiply numerator and denominator by [1 + √(1 - y²)]:

= [ (1 + √(1 - y²))² ] / [1 - (1 - y²)] = [1 + 2√(1 - y²) + 1 - y²] / y² = [2 + 2√(1 - y²) - y²]/y². Hmm, not sure if that helps. Alternatively, perhaps express in terms of inverse hyperbolic functions. Let’s see, ln[(1 + z)/(1 - z)] = 2 artanh(z), where z = √(1 - y²). So the logarithm term is 2 artanh(√(1 - y²)). So the integral becomes 2 ∫₀¹ [2 artanh(√(1 - y²)) * y / (1 - y²)] * K(y) dy. Which is 4 ∫₀¹ [y artanh(√(1 - y²)) / (1 - y²)] K(y) dy. Still not obvious.

Alternatively, maybe use a substitution for artanh(√(1 - y²)). Let’s set w = artanh(√(1 - y²)). Let’s compute dw. Let’s let u = artanh(v), where v = √(1 - y²). Then dv/dy = (1/(2√(1 - y²)))(-2y) = y / √(1 - y²). Then dw/dy = (1/(1 - v²)) * dv/dy. Since v = √(1 - y²), v² = 1 - y². So 1 - v² = y². Therefore, dw/dy = (1/y²) * (y / √(1 - y²)) ) = 1/(y √(1 - y²)). Hmm, but in the integral, we have y artanh(v) / (1 - y²) dy. Let’s see:

The integral is 4 ∫ [artanh(v) * y / (1 - y²)] K(y) dy. Substitute v = √(1 - y²), then 1 - y² = v². So 1 - y² = v² => y² = 1 - v². Then the term y / (1 - y²) = y / v². But y = √(1 - v²). So y / v² = √(1 - v²)/v². Hmm, not sure. Alternatively, express in terms of dw:

From earlier, dw = [1/(y √(1 - y²))] dy. Let’s see, the integral has artanh(v) * y / (1 - y²) dy. Which is artanh(v) * y / (v²) dy. Since 1 - y² = v². So artanh(v) * y / v² dy. But y dy = - v dv, since y² = 1 - v² => 2y dy = -2v dv => y dy = -v dv. Wait, maybe that's useful. Let’s see:

If v = √(1 - y²), then dv/dy = - y / √(1 - y²) = - y / v. So y dy = -v dv. Then, substituting into the integral:

4 ∫ [artanh(v) * y / v²] dy = 4 ∫ artanh(v) * (y / v²) dy. But y dy = -v dv, so dy = -v dv / y. Wait, this might not be straightforward. Let me try:

Express y in terms of v: y = √(1 - v²). So the integral becomes 4 ∫ artanh(v) * [√(1 - v²) / v²] * dy. But we need to express dy in terms of dv. From v = √(1 - y²), we have dv = (-y / √(1 - y²)) dy = (-y / v) dy. Therefore, dy = -v dv / y. Substitute into the integral:

4 ∫ artanh(v) * [√(1 - v²) / v²] * (-v / √(1 - v²)) dv. Simplify terms:

The √(1 - v²) cancels with the denominator, and we have -4 ∫ artanh(v) * (1 / v) dv. So the integral simplifies to -4 ∫ artanh(v) / v dv. But the limits of integration would change. When y goes from 0 to1, v goes from1 to0. So the original limits for v are from1 to0, but with the substitution, we have a negative sign, so the integral becomes:

-4 ∫₁⁰ [artanh(v)/v] dv = 4 ∫₀¹ [artanh(v)/v] dv. So now, the integral reduces to 4 times the integral of artanh(v)/v dv from0 to1. That's a significant simplification! So now, we need to compute ∫₀¹ artanh(v)/v dv.

Let’s compute ∫ artanh(v)/v dv. Let’s recall that artanh(v) = (1/2) ln((1 + v)/(1 - v)). So the integral becomes (1/2) ∫ [ln((1 + v)/(1 - v))]/v dv. Let’s make substitution s = v. Then, expanding the logarithm, we can write it as (1/2) [∫ ln(1 + v)/v dv - ∫ ln(1 - v)/v dv]. These integrals are related to the dilogarithm function. Recall that ∫ ln(1 + v)/v dv = -Li₂(-v) + C and ∫ ln(1 - v)/v dv = -Li₂(v) + C. Therefore, the integral becomes (1/2)[ -Li₂(-v) + Li₂(v) ] + C evaluated from0 to1.

So evaluating from0 to1:

(1/2)[ (-Li₂(-1) + Li₂(1)) - (-Li₂(0) + Li₂(0)) ] = (1/2)[ -Li₂(-1) + Li₂(1) ].

We know that Li₂(1) = π²/6, and Li₂(-1) = -π²/12. Therefore:

(1/2)[ -(-π²/12) + π²/6 ] = (1/2)[ π²/12 + π²/6 ] = (1/2)( π²/12 + 2π²/12 ) = (1/2)(3π²/12) = (1/2)(π²/4) = π²/8.

Therefore, ∫₀¹ artanh(v)/v dv = π²/8. Therefore, the original integral is 4 * π²/8 = π²/2.

Wait, that's a nice result! So the integral simplifies down to π²/2. Let me verify the steps to make sure I didn't make a mistake.

Starting from the original integral, substitution t = √x, leading to 2 ∫₀¹ [ln((1 + t)/(1 - t))/t] * K'(t) dt. Then changing variables to y = √(1 - t²), which transformed the integral into 4 ∫₀¹ [artanh(v)/v] dv, which evaluates to 4*(π²/8) = π²/2. That seems correct.

Let me check the substitution steps again. When we set y = √(1 - t²), then t = √(1 - y²), dt = - y / √(1 - y²) dy. The integral became 4 ∫₀¹ [artanh(√(1 - y²)) * y / (1 - y²)] K(y) dy. Then through substitution and changing variables, we ended up as 4 ∫₀¹ artanh(v)/v dv. That seems correct because all the substitutions canceled out properly, leading to the integral of artanh(v)/v dv, which is known.

Yes, and the integral of artanh(v)/v from0 to1 is π²/8, so multiplying by4 gives π²/2. Therefore, the exact value of the integral is π²/2.

Now, for the numerical approximation. π²/2 is approximately (9.8696044)/2 ≈4.9348022. Rounded to 10 decimal places, that's 4.9348022005. So the numerical approximation is approximately 4.9348022005.

Let me confirm with a quick numerical check. If I compute the original integral numerically, say using a calculator or software, does it give around 4.9348? Given that π²/2 is approximately 4.9348, this seems plausible. So the analytical result is π²/2, and the numerical value is approximately 4.9348022005.
</think>

{"answer": "\\frac{\\pi^2}{2}", "numerical_answer": "4.9348022005"}