# Evaluating the definite integral $\int\sin(101x)\sin(x)^{99}dx$

Let me solve this step by step.

## Step 1: Recognize the pattern
I notice that we have $\sin(101x)$ multiplied by $\sin(x)^{99}$. We need to use trigonometric identities to simplify this.

## Step 2: Use the power-reduction formula for $\sin(x)^{99}$
We know that $\sin^{99}(x)$ is an odd function since 99 is odd. We can express $\sin^{99}(x)$ in terms of sines of multiple angles.

However, there's another approach that's more direct for this integral. Let's use the product-to-sum formula:

$$\sin(A)\sin(B) = \frac{1}{2}[\cos(A-B) - \cos(A+B)]$$

## Step 3: Rewrite the integrand using binomial expansion and product-to-sum formulas

Let's consider the trigonometric identity:
$$\sin^{n}(x) = \frac{1}{2^n}\sum_{k=0}^{n}\binom{n}{k}(-1)^{n-k}\cos(2kx-nx)$$

This is quite complex for n=99, so let's use another approach.

We can write $\sin^{99}(x) = \sin^{98}(x)\sin(x) = (1-\cos^2(x))^{49}\sin(x)$

But this also gets very complicated.

Let's take a different approach using complex exponentials.

## Step 4: Use complex exponentials to solve the integral

We know that $\sin(x) = \frac{e^{ix} - e^{-ix}}{2i}$

So $\sin(101x) = \frac{e^{101ix} - e^{-101ix}}{2i}$

And $\sin^{99}(x) = \left(\frac{e^{ix} - e^{-ix}}{2i}\right)^{99}$

By the binomial theorem:
$$\sin^{99}(x) = \frac{1}{(2i)^{99}}\sum_{k=0}^{99}\binom{99}{k}e^{ix(99-2k)}(-1)^k$$

Multiplying these together and integrating term by term gets very complex.

Let me use a more direct approach with the product-to-sum formula.

## Step 5: Use the identity $\sin(A)\sin(B) = \frac{1}{2}[\cos(A-B) - \cos(A+B)]$

We can use a more general result that when $n$ is odd:

$$\sin(mx)\sin^n(x) = \frac{1}{2^n}\sum_{k=0}^{n/2}(-1)^{n/2-k}\binom{n}{k}\sin((m+n-2k)x)$$

For our case with $n=99$ (odd) and $m=101$:

$$\sin(101x)\sin^{99}(x) = \frac{1}{2^{99}}\sum_{k=0}^{49}(-1)^{49-k}\binom{99}{k}\sin((101+99-2k)x)$$

This simplifies to:

$$\sin(101x)\sin^{99}(x) = \frac{1}{2^{99}}\sum_{k=0}^{49}(-1)^{49-k}\binom{99}{k}\sin((200-2k)x)$$

## Step 6: Integrate each term

For each term, we have:
$$\int \sin((200-2k)x)dx = -\frac{1}{200-2k}\cos((200-2k)x) + C$$

So our integral becomes:
$$\int\sin(101x)\sin^{99}(x)dx = \frac{1}{2^{99}}\sum_{k=0}^{49}(-1)^{49-k}\binom{99}{k}\left(-\frac{1}{200-2k}\cos((200-2k)x)\right) + C$$

Simplifying:
$$\int\sin(101x)\sin^{99}(x)dx = -\frac{1}{2^{99}}\sum_{k=0}^{49}(-1)^{49-k}\binom{99}{k}\frac{\cos((200-2k)x)}{200-2k} + C$$

This is the indefinite integral. Since no limits were provided in the problem, I'll leave the answer in this form.

## Step 7: Final answer

The indefinite integral is:
$$\int\sin(101x)\sin^{99}(x)dx = -\frac{1}{2^{99}}\sum_{k=0}^{49}(-1)^{49-k}\binom{99}{k}\frac{\cos((200-2k)x)}{200-2k} + C$$

For a numerical approximation, we would need specific limits of integration, which weren't provided in the problem. Therefore, I can only provide the exact answer without a numerical value.

Since the question asks for a definite integral but no limits were specified, I'll assume this is an indefinite integral.

{"answer": "-\\frac{1}{2^{99}}\\sum_{k=0}^{49}(-1)^{49-k}\\binom{99}{k}\\frac{\\cos((200-2k)x)}{200-2k} + C", "numerical_answer": "N/A"}