
To solve the definite integral \(\int_{0}^{2} x^{-1/4}(2-x)^{-3/4} \cosh\left(\sqrt[4]{x(2-x)}\right) \, dx\), we proceed as follows:

### Step 1: Substitution and Simplification
First, we use the substitution \(u = \frac{x}{2}\), which transforms \(x = 2u\) and \(dx = 2 \, du\). The limits of integration change from \(x \in [0, 2]\) to \(u \in [0, 1]\). Substituting these into the integral, we get:
\[
\int_{0}^{2} x^{-1/4}(2-x)^{-3/4} \cosh\left(\sqrt[4]{x(2-x)}\right) \, dx = \int_{0}^{1} u^{-1/4}(1-u)^{-3/4} \cosh\left(\sqrt{2} \sqrt[4]{u(1-u)}\right) \, du
\]
where we simplified \(\sqrt[4]{x(2-x)} = \sqrt[4]{4u(1-u)} = \sqrt{2} \sqrt[4]{u(1-u)}\).

### Step 2: Series Expansion of \(\cosh\)
We expand \(\cosh(z)\) as a power series: \(\cosh(z) = \sum_{n=0}^{\infty} \frac{z^{2n}}{(2n)!}\), where \(z = \sqrt{2} \sqrt[4]{u(1-u)}\). Substituting this into the integral, we get:
\[
\int_{0}^{1} u^{-1/4}(1-u)^{-3/4} \sum_{n=0}^{\infty} \frac{(\sqrt{2})^{2n} (u(1-u))^{n/2}}{(2n)!} \, du
\]
Interchanging the sum and integral (justified by uniform convergence), we have:
\[
\sum_{n=0}^{\infty} \frac{2^n}{(2n)!} \int_{0}^{1} u^{n/2 - 1/4}(1-u)^{n/2 - 3/4} \, du
\]

### Step 3: Beta Function and Gamma Function
The integral inside the sum is a Beta function: \(\int_{0}^{1} u^{a-1}(1-u)^{b-1} \, du = B(a, b) = \frac{\Gamma(a)\Gamma(b)}{\Gamma(a+b)}\). Here, \(a = \frac{n}{2} + \frac{3}{4}\) and \(b = \frac{n}{2} + \frac{1}{4}\), so:
\[
B\left(\frac{n}{2} + \frac{3}{4}, \frac{n}{2} + \frac{1}{4}\right) = \frac{\Gamma\left(\frac{n}{2} + \frac{3}{4}\right)\Gamma\left(\frac{n}{2} + \frac{1}{4}\right)}{\Gamma(n + 1)}
\]

### Step 4: Gamma Function Duplication Formula
Using the duplication formula for Gamma functions, \(\Gamma(z)\Gamma\left(z + \frac{1}{2}\right) = 2^{1-2z} \sqrt{\pi} \Gamma(2z)\), we simplify the product of Gamma functions. For \(z = \frac{n}{2} + \frac{1}{4}\), this gives:
\[
\Gamma\left(\frac{n}{2} + \frac{3}{4}\right)\Gamma\left(\frac{n}{2} + \frac{1}{4}\right) = 2^{1/2 - n} \sqrt{\pi} \Gamma\left(n + \frac{1}{2}\right)
\]

### Step 5: Summing the Series
Substituting back and simplifying, the series reduces to a form involving the modified Bessel function \(I_0(1)\). The final result is:
\[
\int_{0}^{2} x^{-1/4}(2-x)^{-3/4} \cosh\left(\sqrt[4]{x(2-x)}\right) \, dx = \sqrt{2} \pi \, I_0(1)
\]

### Step 6: Numerical Approximation
The modified Bessel function \(I_0(1) \approx 1.26606587775\). Thus, the numerical approximation is:
\[
\sqrt{2} \pi \, I_0(1) \approx 5.6213720380
\]

{"answer": "\(\sqrt{2} \pi I_0(1)\)", "numerical_answer": "5.6213720380"}