To compute the definite integral 

\[
\int_0^1 \frac{x - 1}{(x + 1) \ln x} \, dx,
\]

we proceed with the following steps:

### Step 1: Substitution
Let \( x = e^{-t} \). Then, \( dx = -e^{-t} dt \), and the limits change as follows:
- When \( x = 0 \), \( t \to \infty \).
- When \( x = 1 \), \( t = 0 \).

The integral becomes:

\[
\int_{\infty}^0 \frac{e^{-t} - 1}{(e^{-t} + 1) \ln e^{-t}} (-e^{-t}) \, dt = \int_0^{\infty} \frac{e^{-t} - 1}{(e^{-t} + 1)(-t)} e^{-t} \, dt.
\]

Simplifying:

\[
\int_0^{\infty} \frac{(1 - e^{-t}) e^{-t}}{(e^{-t} + 1) t} \, dt = \int_0^{\infty} \frac{e^{-t} - e^{-2t}}{(1 + e^{-t}) t} \, dt.
\]

### Step 2: Series Expansion
Express the denominator \( (1 + e^{-t})^{-1} \) as a geometric series:

\[
\frac{1}{1 + e^{-t}} = \sum_{n=0}^{\infty} (-1)^n e^{-n t}.
\]

Thus, the integrand becomes:

\[
\frac{e^{-t} - e^{-2t}}{t} \sum_{n=0}^{\infty} (-1)^n e^{-n t} = \sum_{n=0}^{\infty} (-1)^n \frac{e^{-(n+1)t} - e^{-(n+2)t}}{t}.
\]

### Step 3: Integrate Term by Term
The integral becomes:

\[
\sum_{n=0}^{\infty} (-1)^n \int_0^{\infty} \frac{e^{-(n+1)t} - e^{-(n+2)t}}{t} \, dt.
\]

Each integral is of the form:

\[
\int_0^{\infty} \frac{e^{-a t} - e^{-b t}}{t} \, dt = \ln \frac{b}{a},
\]

by Frullani's integral. Applying this:

\[
\sum_{n=0}^{\infty} (-1)^n \ln \frac{n+2}{n+1} = \sum_{n=0}^{\infty} (-1)^n \ln \left(1 + \frac{1}{n+1}\right).
\]

### Step 4: Simplify the Series
The series can be recognized as the alternating sum of logarithms:

\[
\ln \prod_{n=0}^{\infty} \left(\frac{2n+2}{2n+1} \cdot \frac{2n+1}{2n+2}\right)^{(-1)^n} = \ln \left(\frac{2}{1} \cdot \frac{1}{2} \cdot \frac{4}{3} \cdot \frac{3}{4} \cdots \right).
\]

This product telescopes to:

\[
\ln \left(\frac{2}{1} \cdot \frac{1}{2} \cdot \frac{4}{3} \cdot \frac{3}{4} \cdots \right) = \ln 1 = 0.
\]

However, this approach seems to lead to a trivial result, which suggests a miscalculation. Instead, let's consider an alternative method.

### Alternative Approach: Differentiation Under the Integral Sign
Consider the parameterized integral:

\[
I(a) = \int_0^1 \frac{x^a - 1}{(x + 1) \ln x} \, dx.
\]

Differentiate with respect to \( a \):

\[
I'(a) = \int_0^1 \frac{x^a}{x + 1} \, dx.
\]

This integral can be evaluated as:

\[
I'(a) = \sum_{n=0}^{\infty} (-1)^n \int_0^1 x^{a + n} \, dx = \sum_{n=0}^{\infty} \frac{(-1)^n}{a + n + 1}.
\]

Integrate \( I'(a) \) from \( a = 0 \) to \( a = 1 \):

\[
I(1) - I(0) = \int_0^1 \sum_{n=0}^{\infty} \frac{(-1)^n}{a + n + 1} \, da = \sum_{n=0}^{\infty} (-1)^n \ln \left(1 + \frac{1}{n + 1}\right).
\]

Since \( I(0) = 0 \), we have:

\[
I(1) = \sum_{n=0}^{\infty} (-1)^n \ln \left(1 + \frac{1}{n + 1}\right).
\]

This series converges to \( \ln \frac{\pi}{2} \), as it is related to the Wallis product.

### Final Answer
The exact value of the integral is:

\[
\ln \frac{\pi}{2}.
\]

A numerical approximation to 10 decimal places is:

\[
0.4515827053.
\]

### JSON Output
```json
{"answer": "\\ln \\frac{\\pi}{2}", "numerical_answer": "0.4515827053"}
```