Let us evaluate the definite integral:

\[
I = \int_{0}^{2} x^{-1/2} (2-x)^{1/2} \left[1 - 0.5x(2-x)\right]^{1/2} \, dx
\]

Let's proceed strictly as requested:

---

### 1. Substitution

Let us consider the substitution:
\[
x = 2\sin^2\theta, \quad x \in [0,2] \implies \theta \in [0, \pi/2]
\]
Then:
\[
dx = 4\sin\theta\cos\theta\, d\theta = 2\sin 2\theta\, d\theta
\]
Now,
\[
x^{-1/2} = (2\sin^2\theta)^{-1/2} = \frac{1}{\sqrt{2}\sin\theta}
\]
\[
2-x = 2(1-\sin^2\theta) = 2\cos^2\theta \implies (2-x)^{1/2} = \sqrt{2}\cos\theta
\]
Now let's compute the remaining factor:
\[
1 - 0.5 x (2-x) = 1 - 0.5 \cdot 2\sin^2\theta \cdot 2\cos^2\theta = 1 - 2\sin^2\theta\cos^2\theta
\]
But
\[
2\sin^2\theta\cos^2\theta = \frac{1}{2}\sin^2 2\theta
\]
So,
\[
1 - 2\sin^2\theta\cos^2\theta = 1 - \frac{1}{2}\sin^2 2\theta
\]

So,
\[
\left[1 - 0.5 x (2-x)\right]^{1/2} = \left[1 - \frac{1}{2}\sin^2 2\theta\right]^{1/2}
\]

Now,
\[
dx = 4\sin\theta\cos\theta\, d\theta = 2\sin 2\theta\, d\theta
\]
So the integral becomes:

\[
I = \int_{x=0}^{x=2} x^{-1/2} (2-x)^{1/2} \left[1 - 0.5 x (2-x)\right]^{1/2}\, dx
= \int_{\theta=0}^{\theta=\pi/2} \frac{1}{\sqrt{2}\sin\theta} \cdot \sqrt{2}\cos\theta \cdot \left[1-\frac{1}{2}\sin^2 2\theta\right]^{1/2} \cdot 4\sin\theta\cos\theta\,d\theta
\]

Prepare the pieces:
- \( \frac{1}{\sqrt{2}\sin\theta} \cdot \sqrt{2}\cos\theta = \frac{\cos\theta}{\sin\theta} \)
- \( 4\sin\theta\cos\theta = 2\sin 2\theta \)

So, putting all together:
\[
I = \int_{0}^{\pi/2} \frac{\cos\theta}{\sin\theta} \left[1-\frac{1}{2}\sin^2 2\theta\right]^{1/2} \cdot 4 \sin\theta \cos\theta\, d\theta
= 4\int_{0}^{\pi/2} \cos^2\theta \left[1-\frac{1}{2}\sin^2 2\theta\right]^{1/2} d\theta
\]

So the integral becomes:

\[
I = 4 \int_{0}^{\pi/2} \cos^2\theta \left[1 - \frac{1}{2} \sin^2 2\theta \right]^{1/2} d\theta
\]

---

### 2. Further simplification

Let’s notice that:
\[
\sin 2\theta = 2\sin\theta\cos\theta
\]
So:
\[
I = 4 \int_{0}^{\pi/2} \cos^2\theta \left[1 - \frac{1}{2} \sin^2 2\theta \right]^{1/2} d\theta
\]

Let’s try substituting \( t = \sin 2\theta \). As \(\theta\) goes from \(0\) to \(\frac{\pi}{2}\), \( t \) goes from \(0\) to \(0\), because \(\sin 2\theta\) is 0 at both endpoints but reaches a maximum of 1 at \(\theta = \pi/4\). This suggests splitting the integration range at \(\theta = \pi/4\):

Let’s also recall that:
\[
\cos^2\theta = \frac{1+\cos 2\theta}{2}
\]

So,
\[
I = 4 \int_{0}^{\pi/2} \frac{1 + \cos 2\theta}{2} \left[1 - \frac{1}{2} \sin^2 2\theta \right]^{1/2} d\theta
= 2 \int_{0}^{\pi/2} (1+\cos 2\theta) \left[1 - \frac{1}{2} \sin^2 2\theta \right]^{1/2} d\theta
\]

Let’s try the substitution \( u = 2\theta \), \(\theta = u/2\), \(d\theta = du/2\), as \(\theta\) goes from \(0\) to \(\frac{\pi}{2}\), \(u\) goes from \(0\) to \(\pi\):

\[
I = 2 \int_{u=0}^{u=\pi} [1 + \cos u] \left[1 - \frac{1}{2} \sin^2 u \right]^{1/2} \frac{du}{2}
\]
\[
= \int_{0}^{\pi} [1+\cos u] \left[1 - \frac{1}{2} \sin^2 u\right]^{1/2} du
\]

Now, split the integral:
\[
I = \int_{0}^{\pi} \left[1-\frac{1}{2} \sin^2 u \right]^{1/2} du + \int_{0}^{\pi} \cos u \left[1-\frac{1}{2} \sin^2 u \right]^{1/2} du
\]

But since \(\left[1-\frac{1}{2} \sin^2 u\right]^{1/2}\) is an even function about \(u = \pi/2\), and \(\cos u\) is odd around \(u = \pi/2\), the second integral is 0, as the function is odd and integrates to 0 over \([0,\pi]\):

\[
\int_{0}^{\pi} f(u)\cos u \, du = 0
\]

Therefore,

\[
I = \int_{0}^{\pi} \left[1-\frac{1}{2} \sin^2 u \right]^{1/2} du
\]

---

### 3. Express in terms of elliptic integrals

We have:

\[
I = \int_{0}^{\pi} \sqrt{1-\frac{1}{2}\sin^2 u} \, du
\]

Recall the standard integral:

\[
\int_{0}^{\pi} \sqrt{1 - k^2 \sin^2 u}\, du = 2 E(k)
\]
where \(E(k)\) is the complete elliptic integral of the second kind, with modulus \(k\):

\[
E(k) = \int_{0}^{\frac{\pi}{2}} \sqrt{1 - k^2 \sin^2 \theta}\, d\theta
\]

In our case, \(k^2 = \frac{1}{2}\), so \(k = \frac{1}{\sqrt{2}}\).

Therefore,

\[
I = 2 E\left( \frac{1}{\sqrt{2}} \right )
\]

---

### 4. Final answer

So the exact answer is:

\[
\boxed{I = 2 E\left( \frac{1}{\sqrt{2}} \right)}
\]

---

### 5. Numerical approximation

Using \( E\left(\frac{1}{\sqrt{2}}\right) \approx 1.350643881047675 \) (from reference tables or WolframAlpha):

So,

\[
I \approx 2 \times 1.350643881047675 = 2.70128776209535
\]

Rounded to 10 decimal places:

\[
I \approx 2.7012877621
\]

---

### 6. JSON output

```json
{"answer": "2 E\\left(\\frac{1}{\\sqrt{2}}\\right)", "numerical_answer": "2.7012877621"}
```