<think>
Okay, so I need to compute the definite integral from 0 to π/2 of [cos²x(1 + cosx)] divided by (1 + cosx + sinx) squared dx. Hmm, let's see. First, I should look for a substitution or some trigonometric identities that can simplify the integrand. The denominator is (1 + cosx + sinx)², which looks a bit complicated. Maybe expanding it or using a substitution could help.

Let me start by simplifying the denominator. Let's denote D = 1 + cosx + sinx. Then the denominator is D². The numerator is cos²x(1 + cosx). So the integrand becomes [cos²x(1 + cosx)] / D². Hmm, perhaps there's a way to express this as a derivative of some function involving D. If I can write the numerator as a combination of D and its derivative, that might help.

First, let's compute the derivative of D with respect to x. D = 1 + cosx + sinx, so D' = -sinx + cosx. That's interesting. Let me see if the numerator can be related to D and D'. Let's see:

The numerator is cos²x(1 + cosx). Let's expand that: cos²x + cos³x. Hmm, not sure. Alternatively, maybe factor something out. Let's see, 1 + cosx is a factor in the numerator. Maybe we can use substitution u = 1 + cosx + sinx, then du/dx = -sinx + cosx. But how does that relate to the numerator?

Alternatively, maybe use a Weierstrass substitution, t = tan(x/2). That sometimes helps with trigonometric integrals. Let me recall that substitution. If t = tan(x/2), then sinx = 2t/(1 + t²), cosx = (1 - t²)/(1 + t²), and dx = 2/(1 + t²) dt. Let's see if that works here.

But before going into that, maybe another approach. Let's consider multiplying numerator and denominator by (1 + cosx - sinx) to rationalize the denominator. Wait, but the denominator is squared, so maybe that's not straightforward. Alternatively, perhaps split the fraction into parts.

Alternatively, let's consider writing the integrand as [cos²x(1 + cosx)] / (1 + cosx + sinx)^2. Let me split the numerator into cos²x times (1 + cosx). Maybe express cos²x in terms of sinx. Since cos²x = 1 - sin²x. So substituting that in, the numerator becomes (1 - sin²x)(1 + cosx). Hmm, but not sure if that helps.

Alternatively, let's try to express the integrand in terms of t = tan(x/2). Let's proceed with that substitution. Let t = tan(x/2), so when x = 0, t = 0, and when x = π/2, t = tan(π/4) = 1. So the limits of integration become from 0 to 1. Then, as per the substitution:

sinx = 2t/(1 + t²)

cosx = (1 - t²)/(1 + t²)

dx = 2/(1 + t²) dt

So let's substitute all these into the integrand.

First, compute the numerator: cos²x(1 + cosx)

cosx = (1 - t²)/(1 + t²), so cos²x = (1 - t²)^2/(1 + t²)^2

1 + cosx = 1 + (1 - t²)/(1 + t²) = [ (1 + t²) + (1 - t²) ] / (1 + t²) ) = 2/(1 + t²)

So the numerator becomes:

(1 - t²)^2/(1 + t²)^2 * 2/(1 + t²) = 2(1 - t²)^2 / (1 + t²)^3

Now the denominator: (1 + cosx + sinx)^2

1 + cosx + sinx = 1 + (1 - t²)/(1 + t²) + 2t/(1 + t²) = [ (1 + t²) + (1 - t²) + 2t ] / (1 + t²) = [1 + t² + 1 - t² + 2t]/(1 + t²) = (2 + 2t)/(1 + t²) = 2(1 + t)/(1 + t²)

Therefore, the denominator squared is [2(1 + t)/(1 + t²)]² = 4(1 + t)^2/(1 + t²)^2

So the integrand becomes:

[2(1 - t²)^2 / (1 + t²)^3] / [4(1 + t)^2/(1 + t²)^2] ] = [2(1 - t²)^2 / (1 + t²)^3] * [ (1 + t²)^2 / 4(1 + t)^2 ) ] = [2(1 - t²)^2 / 4(1 + t)^2(1 + t²) ) ] = [ (1 - t²)^2 ] / [ 2(1 + t)^2(1 + t²) ]

Simplify (1 - t²) = (1 - t)(1 + t), so (1 - t²)^2 = (1 - t)^2(1 + t)^2. Therefore:

[ (1 - t)^2(1 + t)^2 ] / [ 2(1 + t)^2(1 + t²) ) ] = (1 - t)^2 / [ 2(1 + t²) ]

So the integrand simplifies to (1 - t)^2 / [2(1 + t²)].

Therefore, the integral becomes:

∫ from t=0 to t=1 of [ (1 - t)^2 / (2(1 + t²)) ] * [2/(1 + t²) ] dt

Wait, wait, because dx = 2/(1 + t²) dt. So the entire integral is:

Original integrand * dx = [ (1 - t)^2 / (2(1 + t²)) ] * [2/(1 + t²) ] dt = [ (1 - t)^2 / (1 + t²)^2 ] * dt

So the integral simplifies to ∫₀¹ (1 - t)² / (1 + t²)² dt

Hmm, that seems more manageable. Let's compute this integral.

First, expand (1 - t)^2: 1 - 2t + t². So the integrand becomes (1 - 2t + t²)/(1 + t²)^2.

We can split this into three terms:

∫ [1/(1 + t²)^2 - 2t/(1 + t²)^2 + t²/(1 + t²)^2 ] dt

Let's handle each integral separately.

First term: ∫ 1/(1 + t²)^2 dt. The integral of 1/(1 + t²)^2 dt is (t/(2(1 + t²))) + (1/2) arctan t) + C. This is a standard integral.

Second term: ∫ -2t/(1 + t²)^2 dt. Let u = 1 + t², then du = 2t dt, so -2t dt = -du. So this becomes -∫ du/u² = 1/u + C = 1/(1 + t²) + C.

Third term: ∫ t²/(1 + t²)^2 dt. Let's rewrite t² as (1 + t² - 1). So t²/(1 + t²)^2 = (1 + t² - 1)/(1 + t²)^2 = 1/(1 + t²) - 1/(1 + t²)^2. Therefore, the integral becomes ∫ [1/(1 + t²) - 1/(1 + t²)^2 ] dt = arctan t - [ (t/(2(1 + t²)) + (1/2) arctan t ) ] + C.

Putting all three terms together:

First term: (t/(2(1 + t²)) + (1/2) arctan t )

Second term: 1/(1 + t²)

Third term: arctan t - (t/(2(1 + t²)) + (1/2) arctan t )

So combining all three:

First term + Second term + Third term:

[ (t/(2(1 + t²)) + (1/2) arctan t ) ] + [1/(1 + t²)] + [ arctan t - (t/(2(1 + t²)) + (1/2) arctan t ) ]

Simplify term by term:

The first term's t/(2(1 + t²)) cancels with the third term's -t/(2(1 + t²)).

The first term's (1/2 arctan t) and the third term's -1/2 arctan t also cancel.

So we are left with:

1/(1 + t²) + arctan t

Therefore, the integral ∫ (1 - t)^2/(1 + t²)^2 dt from 0 to 1 is [1/(1 + t²) + arctan t] evaluated from 0 to 1.

Compute at t=1: 1/(1 + 1) + arctan(1) = 1/2 + π/4

Compute at t=0: 1/(1 + 0) + arctan(0) = 1 + 0 = 1

Subtracting, the integral is (1/2 + π/4) - 1 = -1/2 + π/4

So the value is π/4 - 1/2.

Wait, but let me check the steps again to make sure I didn't make a mistake. Let's verify the integration steps.

Original integral after substitution became ∫₀¹ (1 - t)^2 / (1 + t²)^2 dt. Then expanding (1 - t)^2 gives 1 - 2t + t². Then split into three integrals:

I1 = ∫1/(1 + t²)^2 dt

I2 = ∫-2t/(1 + t²)^2 dt

I3 = ∫t²/(1 + t²)^2 dt

For I1: The integral of 1/(1 + t²)^2 is indeed (t/(2(1 + t²)) + (1/2) arctan t) + C. Correct.

For I2: Let u = 1 + t², du = 2t dt, so -2t dt = -du. Then ∫-2t/(1 + t²)^2 dt = -∫ du/u² = 1/u + C = 1/(1 + t²) + C. Correct.

For I3: ∫t²/(1 + t²)^2 dt. As I did before, rewrite t² = (1 + t²) - 1. Then split into ∫1/(1 + t²) dt - ∫1/(1 + t²)^2 dt. The first integral is arctan t, the second is the same as I1, which is (t/(2(1 + t²)) + (1/2) arctan t). So I3 = arctan t - [t/(2(1 + t²)) + (1/2) arctan t] + C = (1/2 arctan t - t/(2(1 + t²))) + C. Correct.

So combining all three:

I1 + I2 + I3 = [ (t/(2(1 + t²)) + 1/2 arctan t) ] + [1/(1 + t²)] + [ (1/2 arctan t - t/(2(1 + t²))) ]

Adding these together:

t/(2(1 + t²)) cancels with -t/(2(1 + t²))

1/2 arctan t + 1/2 arctan t = arctan t

Then +1/(1 + t²)

So total is arctan t + 1/(1 + t²). Therefore, evaluated from 0 to 1:

At 1: arctan(1) + 1/(1 + 1) = π/4 + 1/2

At 0: arctan(0) + 1/(1 + 0) = 0 + 1 = 1

Subtracting: (π/4 + 1/2) - 1 = π/4 - 1/2

So the integral is π/4 - 1/2. Therefore, the exact answer is π/4 - 1/2.

Now, let's compute the numerical approximation. π is approximately 3.1415926536, so π/4 ≈ 0.7853981634. Then subtract 1/2 = 0.5. So 0.7853981634 - 0.5 = 0.2853981634. Rounded to 10 decimal places, that's 0.2853981634. Let me verify with a calculator. Alternatively, compute π/4 - 1/2:

π ≈ 3.141592653589793

π/4 ≈ 0.7853981633974483

Subtract 0.5: 0.7853981633974483 - 0.5 = 0.2853981633974483

Rounded to 10 decimal places: 0.2853981634

So the numerical approximation is approximately 0.2853981634.

Therefore, the final answer is π/4 - 1/2, and the numerical value is approximately 0.2853981634.
</think>

{"answer": "\\frac{\\pi}{4} - \\frac{1}{2}", "numerical_answer": 0.2853981634}