We begin with the integral

  I = ∫₀² x^(–1/2) (2–x)^(–1/2)[1 – 0.5·x(2–x)] dx.

Step 1. Change of variable

Let x = 2 sin²θ. Then
  dx = 4 sinθ cosθ dθ.
When x = 0, sin²θ = 0 so θ = 0; when x = 2, sin²θ = 1 so θ = π/2.

Step 2. Transform the factors

We have
  x^(–1/2) = [2 sin²θ]^(–1/2) = (1/√2)(1/sinθ),
  (2–x)^(–1/2) = [2 – 2 sin²θ]^(–1/2) = [2 cos²θ]^(–1/2) = (1/√2)(1/cosθ).
Thus, 
  x^(–1/2)(2–x)^(–1/2) = 1/(2 sinθ cosθ).

Also, note that
  x(2–x) = [2 sin²θ][2 cos²θ] = 4 sin²θ cos²θ,
so the bracket becomes
  1 – 0.5·x(2–x) = 1 – 0.5·4 sin²θ cos²θ = 1 – 2 sin²θ cos²θ.

Step 3. Substitute into the integral

Replacing everything we have:
  I = ∫₀^(π/2) [1/(2 sinθ cosθ)] · [1 – 2 sin²θ cos²θ] · [4 sinθ cosθ dθ].

The factors simplify:
  [1/(2 sinθ cosθ)]·[4 sinθ cosθ] = 2,
so the integrand becomes
  2[1 – 2 sin²θ cos²θ] dθ.

Thus,
  I = 2∫₀^(π/2) [1 – 2 sin²θ cos²θ] dθ.

Step 4. Express sin²θ cos²θ in terms of sin(2θ)

Recall that sin(2θ) = 2 sinθ cosθ, so
  sin²(2θ) = 4 sin²θ cos²θ ⟹ sin²θ cos²θ = sin²(2θ)/4.
Then,
  1 – 2 sin²θ cos²θ = 1 – 2[sin²(2θ)/4] = 1 – sin²(2θ)/2.

Thus, the integral becomes
  I = 2∫₀^(π/2) [1 – (1/2) sin²(2θ)] dθ
    = 2∫₀^(π/2) dθ – ∫₀^(π/2) sin²(2θ) dθ.

Step 5. Evaluate the integrals separately

1. The first integral:
  2∫₀^(π/2) dθ = 2·(π/2) = π.

2. The second integral:
  ∫₀^(π/2) sin²(2θ) dθ.
Use the power-reduction formula:
  sin²(2θ) = [1 – cos(4θ)]/2.
Thus,
  ∫₀^(π/2) sin²(2θ)dθ = (1/2)∫₀^(π/2) [1 – cos(4θ)] dθ
    = (1/2)[θ – (sin4θ)/4]₀^(π/2)
    = (1/2)[(π/2) – 0] = π/4.

Step 6. Combine the results

So,
  I = π – (π/4) = (3π/4).

Step 7. Numerical approximation

Using π ≈ 3.141592653589793,
  (3π/4) ≈ (3×3.141592653589793)/4 ≈ 2.3561944902.

Final answer in JSON format:

{"answer": "\\frac{3\\pi}{4}", "numerical_answer": "2.3561944902"}