To solve the definite integral \(\int_{0}^{1} \frac{x^{3} + x + 1}{3x^{2} - 3x + 4} \, dx\), we follow these steps:

### Step 1: Polynomial Long Division
First, observe that the degree of the numerator (3) is higher than the degree of the denominator (2). We perform polynomial long division to simplify the integrand:

\[
\frac{x^{3} + x + 1}{3x^{2} - 3x + 4}
\]

Divide \(x^3\) by \(3x^2\) to get \(\frac{x}{3}\). Multiply the denominator by \(\frac{x}{3}\) and subtract from the numerator:

\[
x^3 + x + 1 - \left(\frac{x}{3} \cdot (3x^2 - 3x + 4)\right) = x^3 + x + 1 - (x^3 - x^2 + \frac{4x}{3}) = x^2 + \frac{-x}{3} + 1
\]

Now, divide \(x^2\) by \(3x^2\) to get \(\frac{1}{3}\). Multiply the denominator by \(\frac{1}{3}\) and subtract:

\[
x^2 + \frac{-x}{3} + 1 - \left(\frac{1}{3} \cdot (3x^2 - 3x + 4)\right) = x^2 + \frac{-x}{3} + 1 - (x^2 - x + \frac{4}{3}) = \frac{2x}{3} - \frac{1}{3}
\]

Thus, the division yields:

\[
\frac{x^{3} + x + 1}{3x^{2} - 3x + 4} = \frac{x}{3} + \frac{1}{3} + \frac{\frac{2x}{3} - \frac{1}{3}}{3x^{2} - 3x + 4}
\]

Simplify the remainder term:

\[
\frac{\frac{2x}{3} - \frac{1}{3}}{3x^{2} - 3x + 4} = \frac{2x - 1}{9x^{2} - 9x + 12}
\]

So, the integrand becomes:

\[
\frac{x}{3} + \frac{1}{3} + \frac{2x - 1}{9x^{2} - 9x + 12}
\]

### Step 2: Integrate Term by Term
Now, integrate each term separately:

\[
\int_{0}^{1} \left(\frac{x}{3} + \frac{1}{3} + \frac{2x - 1}{9x^{2} - 9x + 12}\right) dx = \frac{1}{3} \int_{0}^{1} x \, dx + \frac{1}{3} \int_{0}^{1} 1 \, dx + \int_{0}^{1} \frac{2x - 1}{9x^{2} - 9x + 12} \, dx
\]

Compute the first two integrals:

\[
\frac{1}{3} \int_{0}^{1} x \, dx = \frac{1}{3} \left[ \frac{x^2}{2} \right]_{0}^{1} = \frac{1}{6}
\]

\[
\frac{1}{3} \int_{0}^{1} 1 \, dx = \frac{1}{3} \left[ x \right]_{0}^{1} = \frac{1}{3}
\]

For the third integral, let \(u = 9x^2 - 9x + 12\). Then \(du = (18x - 9) dx = 9(2x - 1) dx\), so:

\[
\int \frac{2x - 1}{9x^{2} - 9x + 12} \, dx = \frac{1}{9} \int \frac{du}{u} = \frac{1}{9} \ln|u| + C = \frac{1}{9} \ln|9x^2 - 9x + 12| + C
\]

Evaluate from 0 to 1:

\[
\left. \frac{1}{9} \ln(9x^2 - 9x + 12) \right|_{0}^{1} = \frac{1}{9} \left( \ln(12) - \ln(12) \right) = 0
\]

However, let's recheck the substitution for the third integral. The numerator is \(2x - 1\), and the derivative of the denominator is \(18x - 9 = 9(2x - 1)\). Thus, the integral simplifies perfectly:

\[
\int \frac{2x - 1}{9x^2 - 9x + 12} dx = \frac{1}{9} \ln|9x^2 - 9x + 12| + C
\]

Evaluating from 0 to 1:

\[
\frac{1}{9} \left[ \ln(9(1)^2 - 9(1) + 12) - \ln(9(0)^2 - 9(0) + 12) \right] = \frac{1}{9} \left[ \ln(12) - \ln(12) \right] = 0
\]

So, the third integral contributes 0 to the final result.

### Step 3: Combine Results
Adding the results from the first two integrals:

\[
\frac{1}{6} + \frac{1}{3} = \frac{1}{6} + \frac{2}{6} = \frac{3}{6} = \frac{1}{2}
\]

### Step 4: Numerical Approximation
The exact value is \(\frac{1}{2}\). Numerically, this is:

\[
0.5
\]

### Final Answer
```json
{"answer": "\\frac{1}{2}", "numerical_answer": "0.5000000000"}
```