# Evaluating $\int_0^{\frac12}\ln(\sqrt{1-x}-\sqrt{x})\mathrm{d}x$

## Step 1: Simplify the integrand
Let's work with the expression $\ln(\sqrt{1-x}-\sqrt{x})$ first.

$\ln(\sqrt{1-x}-\sqrt{x}) = \ln\left(\frac{(\sqrt{1-x}-\sqrt{x})(\sqrt{1-x}+\sqrt{x})}{(\sqrt{1-x}+\sqrt{x})}\right)$

$= \ln\left(\frac{1-x-x}{(\sqrt{1-x}+\sqrt{x})}\right)$

$= \ln\left(\frac{1-2x}{(\sqrt{1-x}+\sqrt{x})}\right)$

$= \ln(1-2x) - \ln(\sqrt{1-x}+\sqrt{x})$

So, our integral becomes:
$\int_0^{\frac12}\ln(\sqrt{1-x}-\sqrt{x})\mathrm{d}x = \int_0^{\frac12}[\ln(1-2x) - \ln(\sqrt{1-x}+\sqrt{x})]\mathrm{d}x$

$= \int_0^{\frac12}\ln(1-2x)\mathrm{d}x - \int_0^{\frac12}\ln(\sqrt{1-x}+\sqrt{x})\mathrm{d}x$

## Step 2: Evaluate the first integral
For $\int_0^{\frac12}\ln(1-2x)\mathrm{d}x$, let's use the substitution $u = 1-2x$.

When $x = 0$, $u = 1$
When $x = \frac{1}{2}$, $u = 0$
Also, $dx = -\frac{du}{2}$

The integral becomes:
$\int_0^{\frac12}\ln(1-2x)\mathrm{d}x = \int_{1}^{0}\ln(u)\left(-\frac{1}{2}\right)\mathrm{d}u = \frac{1}{2}\int_{0}^{1}\ln(u)\mathrm{d}u$

Using the formula $\int \ln(u)du = u\ln(u) - u + C$, we get:
$\frac{1}{2}\int_{0}^{1}\ln(u)\mathrm{d}u = \frac{1}{2}[u\ln(u) - u]_{0}^{1}$

Note: As $u \to 0$, $u\ln(u) \to 0$ (by L'HÃ´pital's rule or limit evaluation).

$\frac{1}{2}[u\ln(u) - u]_{0}^{1} = \frac{1}{2}[(1\ln(1) - 1) - (0\ln(0) - 0)] = \frac{1}{2}[-1 - 0] = -\frac{1}{2}$

## Step 3: Evaluate the second integral
For $\int_0^{\frac12}\ln(\sqrt{1-x}+\sqrt{x})\mathrm{d}x$, let's substitute $x = \sin^2(t)$.

When $x = 0$, $t = 0$
When $x = \frac{1}{2}$, $t = \frac{\pi}{4}$
Also, $dx = 2\sin(t)\cos(t)dt = \sin(2t)dt$

With this substitution:
$\sqrt{1-x} = \sqrt{1-\sin^2(t)} = \sqrt{\cos^2(t)} = \cos(t)$
$\sqrt{x} = \sqrt{\sin^2(t)} = \sin(t)$

So, $\sqrt{1-x} + \sqrt{x} = \cos(t) + \sin(t) = \sqrt{2}\sin(t + \frac{\pi}{4})$

The second integral becomes:
$\int_0^{\frac12}\ln(\sqrt{1-x}+\sqrt{x})\mathrm{d}x = \int_{0}^{\frac{\pi}{4}}\ln(\sqrt{2}\sin(t + \frac{\pi}{4}))\sin(2t)\mathrm{d}t$

$= \int_{0}^{\frac{\pi}{4}}[\ln(\sqrt{2}) + \ln(\sin(t + \frac{\pi}{4}))]\sin(2t)\mathrm{d}t$

$= \ln(\sqrt{2})\int_{0}^{\frac{\pi}{4}}\sin(2t)\mathrm{d}t + \int_{0}^{\frac{\pi}{4}}\ln(\sin(t + \frac{\pi}{4}))\sin(2t)\mathrm{d}t$

For the first part:
$\ln(\sqrt{2})\int_{0}^{\frac{\pi}{4}}\sin(2t)\mathrm{d}t = \ln(\sqrt{2})[-\frac{\cos(2t)}{2}]_{0}^{\frac{\pi}{4}}$
$= \ln(\sqrt{2})[-\frac{\cos(\frac{\pi}{2})}{2} + \frac{\cos(0)}{2}]$
$= \ln(\sqrt{2})[-\frac{0}{2} + \frac{1}{2}] = \frac{\ln(\sqrt{2})}{2} = \frac{\ln(2)}{4}$

For the second part, let's substitute $v = t + \frac{\pi}{4}$:
$\int_{0}^{\frac{\pi}{4}}\ln(\sin(t + \frac{\pi}{4}))\sin(2t)\mathrm{d}t = \int_{\frac{\pi}{4}}^{\frac{\pi}{2}}\ln(\sin(v))\sin(2v - \frac{\pi}{2})\mathrm{d}v$

$= \int_{\frac{\pi}{4}}^{\frac{\pi}{2}}\ln(\sin(v))\cos(2v)\mathrm{d}v$

Using integration by parts with $u = \ln(\sin(v))$ and $dv = \cos(2v)dv$:

$\int_{\frac{\pi}{4}}^{\frac{\pi}{2}}\ln(\sin(v))\cos(2v)\mathrm{d}v = \left[\ln(\sin(v))\frac{\sin(2v)}{2}\right]_{\frac{\pi}{4}}^{\frac{\pi}{2}} - \int_{\frac{\pi}{4}}^{\frac{\pi}{2}}\frac{\cos(v)}{\sin(v)}\frac{\sin(2v)}{2}\mathrm{d}v$

$= \left[\ln(\sin(v))\frac{\sin(2v)}{2}\right]_{\frac{\pi}{4}}^{\frac{\pi}{2}} - \int_{\frac{\pi}{4}}^{\frac{\pi}{2}}\frac{\cos(v) \cdot 2\sin(v)\cos(v)}{2\sin(v)}\mathrm{d}v$

$= \left[\ln(\sin(v))\frac{\sin(2v)}{2}\right]_{\frac{\pi}{4}}^{\frac{\pi}{2}} - \int_{\frac{\pi}{4}}^{\frac{\pi}{2}}\cos^2(v)\mathrm{d}v$

Evaluating the first term:
$\left[\ln(\sin(v))\frac{\sin(2v)}{2}\right]_{\frac{\pi}{4}}^{\frac{\pi}{2}} = \ln(\sin(\frac{\pi}{2}))\frac{\sin(\pi)}{2} - \ln(\sin(\frac{\pi}{4}))\frac{\sin(\frac{\pi}{2})}{2}$
$= \ln(1) \cdot 0 - \ln(\frac{1}{\sqrt{2}}) \cdot \frac{1}{2} = -\ln(\frac{1}{\sqrt{2}}) \cdot \frac{1}{2} = \frac{\ln(\sqrt{2})}{2} = \frac{\ln(2)}{4}$

For the second term:
$\int_{\frac{\pi}{4}}^{\frac{\pi}{2}}\cos^2(v)\mathrm{d}v = \int_{\frac{\pi}{4}}^{\frac{\pi}{2}}\frac{1 + \cos(2v)}{2}\mathrm{d}v$
$= \left[\frac{v}{2} + \frac{\sin(2v)}{4}\right]_{\frac{\pi}{4}}^{\frac{\pi}{2}}$
$= \left[\frac{\frac{\pi}{2}}{2} + \frac{\sin(\pi)}{4}\right] - \left[\frac{\frac{\pi}{4}}{2} + \frac{\sin(\frac{\pi}{2})}{4}\right]$
$= \frac{\pi}{4} + 0 - \frac{\pi}{8} - \frac{1}{4} = \frac{\pi}{8} - \frac{1}{4}$

So, the second part of the integral is:
$\frac{\ln(2)}{4} - (\frac{\pi}{8} - \frac{1}{4}) = \frac{\ln(2)}{4} - \frac{\pi}{8} + \frac{1}{4}$

## Step 4: Combine the results
Now, we combine the results from both integrals:

$\int_0^{\frac12}\ln(\sqrt{1-x}-\sqrt{x})\mathrm{d}x = \int_0^{\frac12}\ln(1-2x)\mathrm{d}x - \int_0^{\frac12}\ln(\sqrt{1-x}+\sqrt{x})\mathrm{d}x$

$= -\frac{1}{2} - \left(\frac{\ln(2)}{4} + \frac{\ln(2)}{4} - \frac{\pi}{8} + \frac{1}{4}\right)$

$= -\frac{1}{2} - \frac{\ln(2)}{2} + \frac{\pi}{8} - \frac{1}{4}$

$= -\frac{1}{2} - \frac{1}{4} - \frac{\ln(2)}{2} + \frac{\pi}{8}$

$= -\frac{3}{4} - \frac{\ln(2)}{2} + \frac{\pi}{8}$

$= \frac{\pi}{8} - \frac{3}{4} - \frac{\ln(2)}{2}$

## Step 5: Numerical approximation
Computing the numerical value to 10 decimal places:
$\frac{\pi}{8} - \frac{3}{4} - \frac{\ln(2)}{2} \approx 0.3926990817 - 0.75 - 0.3465735903 \approx -0.7038745086$

{"answer": "\\frac{\\pi}{8} - \\frac{3}{4} - \\frac{\\ln(2)}{2}", "numerical_answer": "-0.7038745086"}