Let's compute the integral:
\[
I = \int_0^1 x \arccos x \, I_0(2x) \, dx
\]
where \( I_0 \) is the modified Bessel function of the first kind.

---

### Step 1: Analytical Solution

#### 1.1. Integration by Parts

Let:
- \( u = \arccos x \implies du = -\frac{1}{\sqrt{1-x^2}} dx \)
- \( dv = x I_0(2x) dx \implies v = \int x I_0(2x) dx \)

Let's compute \( v \):

Let’s use integration by parts for \( \int x I_0(2x) dx \):

Let \( w = x \), \( dz = I_0(2x) dx \).

But it's easier to recall that:
\[
\frac{d}{dx} I_1(2x) = 2 I_0(2x)
\]
So,
\[
I_1(2x) = \int 2 I_0(2x) dx \implies \int I_0(2x) dx = \frac{1}{2} I_1(2x)
\]

Now, integrate by parts:
\[
\int x I_0(2x) dx
\]
Let’s use the reduction formula for Bessel functions:
\[
\frac{d}{dx} [x I_1(2x)] = I_1(2x) + x \cdot 2 I_0(2x) = I_1(2x) + 2x I_0(2x)
\]
So,
\[
2x I_0(2x) = \frac{d}{dx} [x I_1(2x)] - I_1(2x)
\]
\[
x I_0(2x) = \frac{1}{2} \frac{d}{dx} [x I_1(2x)] - \frac{1}{2} I_1(2x)
\]
Therefore,
\[
\int x I_0(2x) dx = \frac{1}{2} x I_1(2x) - \frac{1}{2} \int I_1(2x) dx
\]
But,
\[
\int I_1(2x) dx = \frac{1}{2} I_0(2x)
\]
So,
\[
\int x I_0(2x) dx = \frac{1}{2} x I_1(2x) - \frac{1}{4} I_0(2x)
\]

Thus,
\[
v = \frac{1}{2} x I_1(2x) - \frac{1}{4} I_0(2x)
\]

---

#### 1.2. Apply Integration by Parts

\[
I = \left[ \arccos x \cdot \left( \frac{1}{2} x I_1(2x) - \frac{1}{4} I_0(2x) \right) \right]_0^1 - \int_0^1 \left( \frac{1}{2} x I_1(2x) - \frac{1}{4} I_0(2x) \right) \cdot \left( -\frac{1}{\sqrt{1-x^2}} \right) dx
\]
\[
= \left[ \arccos x \cdot \left( \frac{1}{2} x I_1(2x) - \frac{1}{4} I_0(2x) \right) \right]_0^1 + \int_0^1 \frac{1}{2} x I_1(2x) \frac{dx}{\sqrt{1-x^2}} - \int_0^1 \frac{1}{4} I_0(2x) \frac{dx}{\sqrt{1-x^2}}
\]

---

#### 1.3. Evaluate the Boundary Terms

At \( x = 1 \):
- \( \arccos 1 = 0 \)
- \( x I_1(2x) = I_1(2) \)
- \( I_0(2x) = I_0(2) \)

So, the term is \( 0 \).

At \( x = 0 \):
- \( \arccos 0 = \frac{\pi}{2} \)
- \( x I_1(0) = 0 \)
- \( I_0(0) = 1 \)

So, the term is:
\[
- \frac{\pi}{2} \cdot \frac{1}{4} \cdot 1 = -\frac{\pi}{8}
\]

So, the boundary term is:
\[
0 - \left( -\frac{\pi}{8} \right) = \frac{\pi}{8}
\]

---

#### 1.4. The Remaining Integrals

So,
\[
I = \frac{\pi}{8} + \frac{1}{2} \int_0^1 \frac{x I_1(2x)}{\sqrt{1-x^2}} dx - \frac{1}{4} \int_0^1 \frac{I_0(2x)}{\sqrt{1-x^2}} dx
\]

Let’s compute these two integrals.

---

#### 1.5. Substitute \( x = \sin \theta \), \( dx = \cos \theta d\theta \), \( \sqrt{1-x^2} = \cos \theta \), \( x \in [0,1] \implies \theta \in [0, \pi/2] \):

- \( x = \sin \theta \)
- \( dx = \cos \theta d\theta \)
- \( \sqrt{1-x^2} = \cos \theta \)

So,
\[
\int_0^1 \frac{x I_1(2x)}{\sqrt{1-x^2}} dx = \int_0^{\pi/2} \frac{\sin \theta I_1(2 \sin \theta)}{\cos \theta} \cos \theta d\theta = \int_0^{\pi/2} \sin \theta I_1(2 \sin \theta) d\theta
\]

\[
\int_0^1 \frac{I_0(2x)}{\sqrt{1-x^2}} dx = \int_0^{\pi/2} I_0(2 \sin \theta) d\theta
\]

---

#### 1.6. Known Integrals

From standard tables (see Gradshteyn & Ryzhik 6.671):

\[
\int_0^{\pi/2} I_0(a \sin \theta) d\theta = \frac{\pi}{2} {}_0F_1\left(;1;\frac{a^2}{4}\right)
\]
where \( {}_0F_1 \) is the confluent hypergeometric limit function.

For \( a = 2 \):
\[
\int_0^{\pi/2} I_0(2 \sin \theta) d\theta = \frac{\pi}{2} {}_0F_1\left(;1;1\right)
\]

But \( {}_0F_1(;1;z) = \sum_{k=0}^\infty \frac{z^k}{(k!)^2} \), which is the series for \( I_0(2\sqrt{z}) \) at \( z=1 \), but let's keep it as is for now.

For the other integral, from Gradshteyn & Ryzhik 6.671.6:
\[
\int_0^{\pi/2} \sin \theta I_1(a \sin \theta) d\theta = \frac{\pi}{2a} I_1(a)
\]
For \( a = 2 \):
\[
\int_0^{\pi/2} \sin \theta I_1(2 \sin \theta) d\theta = \frac{\pi}{4} I_1(2)
\]

---

#### 1.7. Substitute Back

So,
\[
I = \frac{\pi}{8} + \frac{1}{2} \cdot \frac{\pi}{4} I_1(2) - \frac{1}{4} \cdot \frac{\pi}{2} {}_0F_1\left(;1;1\right)
\]
\[
= \frac{\pi}{8} + \frac{\pi}{8} I_1(2) - \frac{\pi}{8} {}_0F_1\left(;1;1\right)
\]
\[
= \frac{\pi}{8} \left[ 1 + I_1(2) - {}_0F_1\left(;1;1\right) \right]
\]

But \( {}_0F_1(;1;1) = \sum_{k=0}^\infty \frac{1}{(k!)^2} \), which is the value of \( I_0(2) \), since
\[
I_0(2) = \sum_{k=0}^\infty \frac{1}{(k!)^2}
\]
So,
\[
{}_0F_1(;1;1) = I_0(2)
\]

Therefore,
\[
I = \frac{\pi}{8} \left[ 1 + I_1(2) - I_0(2) \right]
\]

---

### Step 2: Numerical Approximation

Let’s compute the values:

- \( I_0(2) \approx 2.279585302 \)
- \( I_1(2) \approx 1.590636855 \)
- \( \pi \approx 3.141592654 \)

So,
\[
I = \frac{3.141592654}{8} \left[ 1 + 1.590636855 - 2.279585302 \right]
\]
\[
= 0.3926990817 \times (1 + 1.590636855 - 2.279585302)
\]
\[
= 0.3926990817 \times (2.590636855 - 2.279585302)
\]
\[
= 0.3926990817 \times 0.311051553
\]
\[
\approx 0.1220908762
\]

---

### Final Answer

```json
{"answer": "\\frac{\\pi}{8} \\left[ 1 + I_1(2) - I_0(2) \\right]", "numerical_answer": "0.1220908762"}
```