# Evaluation of $\int_0^{\pi/4}\frac{\tan(x)+2\sec^2(x)+2\tan(x)\sec^2(x)}{\tan(x)+\sec^2(x)}\text{ dx}$

I'll solve this definite integral step by step.

## Step 1: Simplify the integrand

Let's start by simplifying the expression in the numerator and denominator:

$$\frac{\tan(x)+2\sec^2(x)+2\tan(x)\sec^2(x)}{\tan(x)+\sec^2(x)}$$

Let's denote $u = \tan(x)$ and $v = \sec^2(x)$ to make this clearer:

$$\frac{u+2v+2uv}{u+v}$$

We can factor the numerator:

$$\frac{u+2v+2uv}{u+v} = \frac{u(1+2v)+2v}{u+v}$$

This can be rewritten as:

$$\frac{u(1+2v)+2v}{u+v} = \frac{u+2uv+2v}{u+v}$$

Now let's try a different approach. Let's expand by dividing each term in the numerator by the denominator:

$$\frac{\tan(x)+2\sec^2(x)+2\tan(x)\sec^2(x)}{\tan(x)+\sec^2(x)} = \frac{\tan(x)}{\tan(x)+\sec^2(x)} + \frac{2\sec^2(x)}{\tan(x)+\sec^2(x)} + \frac{2\tan(x)\sec^2(x)}{\tan(x)+\sec^2(x)}$$

## Step 2: Notice an important relation

Recall that $\sec^2(x) = 1 + \tan^2(x)$. So $\tan(x) + \sec^2(x) = \tan(x) + 1 + \tan^2(x) = 1 + \tan(x) + \tan^2(x)$.

Also note that $\tan(x)\sec^2(x) = \tan(x)(1 + \tan^2(x)) = \tan(x) + \tan^3(x)$.

## Step 3: Use substitution $u = \tan(x)$

Let's use the substitution $u = \tan(x)$, which gives $du = \sec^2(x) dx$.

This means $dx = \frac{du}{\sec^2(x)}$.

When $x = 0$, $u = \tan(0) = 0$.
When $x = \pi/4$, $u = \tan(\pi/4) = 1$.

With this substitution, we have:
$$\sec^2(x) = 1 + u^2$$

So our integral becomes:
$$\int_0^1 \frac{u+2(1+u^2)+2u(1+u^2)}{u+(1+u^2)} \cdot \frac{1}{1+u^2} du$$

Simplifying the numerator:
$$u+2+2u^2+2u+2u^3 = 2+3u+2u^2+2u^3$$

And the denominator:
$$[u+(1+u^2)] \cdot (1+u^2) = (1+u+u^2)(1+u^2) = (1+u^2) + u(1+u^2) = 1+u^2+u+u^3$$

So our integral is:
$$\int_0^1 \frac{2+3u+2u^2+2u^3}{1+u+u^2+u^3} du$$

## Step 4: Further simplification

Let's try polynomial division to simplify the integrand:

$$\frac{2+3u+2u^2+2u^3}{1+u+u^2+u^3} = 2 + \frac{u-0u^2-0u^3}{1+u+u^2+u^3} = 2 + \frac{u}{1+u+u^2+u^3}$$

So our integral becomes:
$$\int_0^1 \left(2 + \frac{u}{1+u+u^2+u^3}\right) du = 2u \bigg|_0^1 + \int_0^1 \frac{u}{1+u+u^2+u^3} du$$

$$= 2 + \int_0^1 \frac{u}{1+u+u^2+u^3} du$$

## Step 5: Factoring the denominator

We need to factor $1+u+u^2+u^3$. Note that $1+u^3 = (1+u)(1-u+u^2)$, so:
$$1+u+u^2+u^3 = 1+u+u^2+u^3 = (1+u)(1+u^2)$$

Wait, that's not correct. Let's try again:
$$1+u+u^2+u^3 = 1+u+u^2+u^3$$

We can check if this factors as $(1+u)(1+u^2)$:
$$(1+u)(1+u^2) = 1+u^2+u+u^3 = 1+u+u^2+u^3$$

Great, so $1+u+u^2+u^3 = (1+u)(1+u^2)$.

So our integral becomes:
$$2 + \int_0^1 \frac{u}{(1+u)(1+u^2)} du$$

## Step 6: Partial fraction decomposition

Let's decompose $\frac{u}{(1+u)(1+u^2)}$ using partial fractions:

$$\frac{u}{(1+u)(1+u^2)} = \frac{A}{1+u} + \frac{Bu+C}{1+u^2}$$

Multiplying both sides by $(1+u)(1+u^2)$:
$$u = A(1+u^2) + (Bu+C)(1+u)$$
$$u = A + Au^2 + Bu + C + Bu^2 + Cu$$
$$u = A + C + (B+C)u + (A+B)u^2$$

Comparing coefficients:
$A + C = 0$
$B + C = 1$
$A + B = 0$

From the third equation: $B = -A$
Substituting into the second: $-A + C = 1$, so $C - A = 1$
From the first equation: $A + C = 0$, so $C = -A$

Combining: $-A - A = 1$ which gives $A = -\frac{1}{2}$
Therefore, $B = \frac{1}{2}$ and $C = \frac{1}{2}$

So we have:
$$\frac{u}{(1+u)(1+u^2)} = \frac{-\frac{1}{2}}{1+u} + \frac{\frac{1}{2}u+\frac{1}{2}}{1+u^2}$$

## Step 7: Integrate each term

Our integral becomes:
$$2 + \int_0^1 \left(\frac{-\frac{1}{2}}{1+u} + \frac{\frac{1}{2}u+\frac{1}{2}}{1+u^2}\right) du$$

$$= 2 - \frac{1}{2}\int_0^1 \frac{1}{1+u} du + \frac{1}{2}\int_0^1 \frac{u}{1+u^2} du + \frac{1}{2}\int_0^1 \frac{1}{1+u^2} du$$

Evaluating each integral:
- $\int \frac{1}{1+u} du = \ln|1+u| + C_1$
- $\int \frac{u}{1+u^2} du = \frac{1}{2}\ln|1+u^2| + C_2$
- $\int \frac{1}{1+u^2} du = \arctan(u) + C_3$

So our integral is:
$$2 - \frac{1}{2}[\ln|1+u|]_0^1 + \frac{1}{2}[\frac{1}{2}\ln|1+u^2|]_0^1 + \frac{1}{2}[\arctan(u)]_0^1$$

$$= 2 - \frac{1}{2}[\ln(2) - \ln(1)] + \frac{1}{4}[\ln(2) - \ln(1)] + \frac{1}{2}[\arctan(1) - \arctan(0)]$$

$$= 2 - \frac{1}{2}\ln(2) + \frac{1}{4}\ln(2) + \frac{1}{2}[\frac{\pi}{4} - 0]$$

$$= 2 - \frac{1}{2}\ln(2) + \frac{1}{4}\ln(2) + \frac{\pi}{8}$$

$$= 2 - \frac{1}{4}\ln(2) + \frac{\pi}{8}$$

## Step 8: Compute the numerical value

The exact value is $2 - \frac{1}{4}\ln(2) + \frac{\pi}{8}$

For the numerical approximation:
- $\ln(2) \approx 0.6931471806$
- $\frac{\pi}{8} \approx 0.3926990817$

So $2 - \frac{1}{4}\ln(2) + \frac{\pi}{8} \approx 2 - 0.1732867952 + 0.3926990817 \approx 2.2194122865$

Therefore, the definite integral evaluates to $2 - \frac{1}{4}\ln(2) + \frac{\pi}{8} \approx 2.2194122865$

{"answer": "2 - \\frac{1}{4}\\ln(2) + \\frac{\\pi}{8}", "numerical_answer": "2.2194122865"}