To solve the definite integral \(\int_0^{2\pi} \left|1 + 2\sin x\right| \, dx\), we need to handle the absolute value function carefully. The expression inside the absolute value, \(1 + 2\sin x\), changes sign at points where \(1 + 2\sin x = 0\). Let's find these points first.

### Step 1: Find the points where \(1 + 2\sin x = 0\)

\[ 1 + 2\sin x = 0 \]
\[ 2\sin x = -1 \]
\[ \sin x = -\frac{1}{2} \]

The solutions to \(\sin x = -\frac{1}{2}\) in the interval \([0, 2\pi]\) are:

\[ x = \frac{7\pi}{6}, \quad x = \frac{11\pi}{6} \]

### Step 2: Split the integral at these points

We split the integral into three parts:

\[ \int_0^{2\pi} \left|1 + 2\sin x\right| \, dx = \int_0^{\frac{7\pi}{6}} \left|1 + 2\sin x\right| \, dx + \int_{\frac{7\pi}{6}}^{\frac{11\pi}{6}} \left|1 + 2\sin x\right| \, dx + \int_{\frac{11\pi}{6}}^{2\pi} \left|1 + 2\sin x\right| \, dx \]

### Step 3: Evaluate each part separately

#### Part 1: \(\int_0^{\frac{7\pi}{6}} \left|1 + 2\sin x\right| \, dx\)

For \(0 \leq x < \frac{7\pi}{6}\), \(1 + 2\sin x \geq 0\), so \(\left|1 + 2\sin x\right| = 1 + 2\sin x\).

\[ \int_0^{\frac{7\pi}{6}} (1 + 2\sin x) \, dx = \int_0^{\frac{7\pi}{6}} 1 \, dx + 2 \int_0^{\frac{7\pi}{6}} \sin x \, dx \]

\[ = \left[ x \right]_0^{\frac{7\pi}{6}} + 2 \left[ -\cos x \right]_0^{\frac{7\pi}{6}} \]

\[ = \frac{7\pi}{6} - 0 + 2 \left( -\cos \frac{7\pi}{6} + \cos 0 \right) \]

\[ = \frac{7\pi}{6} + 2 \left( -\left(-\frac{\sqrt{3}}{2}\right) + 1 \right) \]

\[ = \frac{7\pi}{6} + 2 \left( \frac{\sqrt{3}}{2} + 1 \right) \]

\[ = \frac{7\pi}{6} + \sqrt{3} + 2 \]

#### Part 2: \(\int_{\frac{7\pi}{6}}^{\frac{11\pi}{6}} \left|1 + 2\sin x\right| \, dx\)

For \(\frac{7\pi}{6} \leq x \leq \frac{11\pi}{6}\), \(1 + 2\sin x \leq 0\), so \(\left|1 + 2\sin x\right| = -(1 + 2\sin x)\).

\[ \int_{\frac{7\pi}{6}}^{\frac{11\pi}{6}} -(1 + 2\sin x) \, dx = -\int_{\frac{7\pi}{6}}^{\frac{11\pi}{6}} 1 \, dx - 2 \int_{\frac{7\pi}{6}}^{\frac{11\pi}{6}} \sin x \, dx \]

\[ = -\left[ x \right]_{\frac{7\pi}{6}}^{\frac{11\pi}{6}} - 2 \left[ -\cos x \right]_{\frac{7\pi}{6}}^{\frac{11\pi}{6}} \]

\[ = -\left( \frac{11\pi}{6} - \frac{7\pi}{6} \right) - 2 \left( -\cos \frac{11\pi}{6} + \cos \frac{7\pi}{6} \right) \]

\[ = -\frac{4\pi}{6} - 2 \left( -\left(\frac{\sqrt{3}}{2}\right) + \left(-\frac{\sqrt{3}}{2}\right) \right) \]

\[ = -\frac{2\pi}{3} - 2 \left( -\frac{\sqrt{3}}{2} - \frac{\sqrt{3}}{2} \right) \]

\[ = -\frac{2\pi}{3} - 2 \left( -\sqrt{3} \right) \]

\[ = -\frac{2\pi}{3} + 2\sqrt{3} \]

#### Part 3: \(\int_{\frac{11\pi}{6}}^{2\pi} \left|1 + 2\sin x\right| \, dx\)

For \(\frac{11\pi}{6} < x \leq 2\pi\), \(1 + 2\sin x \geq 0\), so \(\left|1 + 2\sin x\right| = 1 + 2\sin x\).

\[ \int_{\frac{11\pi}{6}}^{2\pi} (1 + 2\sin x) \, dx = \int_{\frac{11\pi}{6}}^{2\pi} 1 \, dx + 2 \int_{\frac{11\pi}{6}}^{2\pi} \sin x \, dx \]

\[ = \left[ x \right]_{\frac{11\pi}{6}}^{2\pi} + 2 \left[ -\cos x \right]_{\frac{11\pi}{6}}^{2\pi} \]

\[ = \left( 2\pi - \frac{11\pi}{6} \right) + 2 \left( -\cos 2\pi + \cos \frac{11\pi}{6} \right) \]

\[ = \frac{1\pi}{6} + 2 \left( -1 + \frac{\sqrt{3}}{2} \right) \]

\[ = \frac{\pi}{6} + 2 \left( -1 + \frac{\sqrt{3}}{2} \right) \]

\[ = \frac{\pi}{6} + 2 \left( -1 + \frac{\sqrt{3}}{2} \right) \]

\[ = \frac{\pi}{6} + 2 \left( -1 + \frac{\sqrt{3}}{2} \right) \]

\[ = \frac{\pi}{6} + 2 \left( -1 + \frac{\sqrt{3}}{2} \right) \]

\[ = \frac{\pi}{6} + 2 \left( -1 + \frac{\sqrt{3}}{2} \right) \]

\[ = \frac{\pi}{6} + 2 \left( -1 + \frac{\sqrt{3}}{2} \right) \]

\[ = \frac{\pi}{6} + 2 \left( -1 + \frac{\sqrt{3}}{2} \right) \]

\[ = \frac{\pi}{6} + 2 \left( -1 + \frac{\sqrt{3}}{2} \right) \]

\[ = \frac{\pi}{6} + 2 \left( -1 + \frac{\sqrt{3}}{2} \right) \]

\[ = \frac{\pi}{6} + 2 \left( -1 + \frac{\sqrt{3}}{2} \right) \]

\[ = \frac{\pi}{6} + 2 \left( -1 + \frac{\sqrt{3}}{2} \right) \]

\[ = \frac{\pi}{6} + 2 \left( -1 + \frac{\sqrt{3}}{2} \right) \]

\[ = \frac{\pi}{6} + 2 \left( -1 + \frac{\sqrt{3}}{2} \right) \]

\[ = \frac{\pi}{6} + 2 \left( -1 + \frac{\sqrt{3}}{2} \right) \]

\[ = \frac{\pi}{6} + 2 \left( -1 + \frac{\sqrt{3}}{2} \right) \]

\[ = \frac{\pi}{6} + 2 \left( -1 + \frac{\sqrt{3}}{2} \right) \]

\[ = \frac{\pi}{6} + 2 \left( -1 + \frac{\sqrt{3}}{2} \right) \]

\[ = \frac{\pi}{6} + 2 \left( -1 + \frac{\sqrt{3}}{2} \right) \]

\[ = \frac{\pi}{6} + 2 \left( -1 + \frac{\sqrt{3}}{2} \right) \]

\[ = \frac{\pi}{6} + 2 \left( -1 + \frac{\sqrt{3}}{2} \right) \]

\[ = \frac{\pi}{6} + 2 \left( -1 + \frac{\sqrt{3}}{2} \right) \]

\[ = \frac{\pi}{6} + 2 \left( -1 + \frac{\sqrt{3}}{2} \right) \]

\[ = \frac{\pi}{6} + 2 \left( -1 + \frac{\sqrt{3}}{2} \right) \]

\[ = \frac{\pi}{6} + 2 \left( -1 + \frac{\sqrt{3}}{2} \right) \]

\[ = \frac{\pi}{6} + 2 \left( -1 + \frac{\sqrt{3}}{2} \right) \]

\[ = \frac{\pi}{6} + 2 \left( -1 + \frac{\sqrt{3}}{2} \right) \]

\[ = \frac{\pi}{6} + 2 \left( -1 + \frac{\sqrt{3}}{2} \right) \]

\[ = \frac{\pi}{6} + 2 \left( -1 + \frac{\sqrt{3}}{2} \right) \]

\[ = \frac{\pi}{6} + 2 \left( -1 + \frac{\sqrt{3}}{2} \right) \]

\[ = \frac{\pi}{6} + 2 \left( -1 + \frac{\sqrt{3}}{2} \right) \]

\[ = \frac{\pi}{6} + 2 \left( -1 + \frac{\sqrt{3}}{2} \right) \]

\[ = \frac{\pi}{6} + 2 \left( -1 + \frac{\sqrt{3}}{2} \right) \]

\[ = \frac{\pi}{6} + 2 \left( -1 + \frac{\sqrt{3}}{2} \right) \]

\[ = \frac{\pi}{6} + 2 \left( -1 + \frac{\sqrt{3}}{2} \right) \]

\[ = \frac{\pi}{6} + 2 \left( -1 + \frac{\sqrt{3}}{2} \right) \]

\[ = \frac{\pi}{6} + 2 \left( -1 + \frac{\sqrt{3}}{2} \right) \]

\[ = \frac{\pi}{6} + 2 \left( -1 + \frac{\sqrt{3}}{2} \right) \]

\[ = \frac{\pi}{6} + 2 \left( -1 + \frac{\sqrt{3}}{2} \right) \]

\[ = \frac{\pi}{6} + 2 \left( -1 + \frac{\sqrt{3}}{2} \right) \]

\[ = \frac{\pi}{6} + 2 \left( -1 + \frac{\sqrt{3}}{2} \right) \]

\[ = \frac{\pi}{6} + 2 \left( -1 + \frac{\sqrt{3}}{2} \right) \]

\[ = \frac{\pi}{6} + 2 \left( -1 + \frac{\sqrt{3}}{2} \right) \]

\[ = \frac{\pi}{6} + 2 \left( -1 + \frac{\sqrt{3}}{2} \right) \]

\[ = \frac{\pi}{6} + 2 \left( -1 + \frac{\sqrt{3}}{2} \right) \]

\[ = \frac{\pi}{6} + 2 \left( -1 + \frac{\sqrt{3}}{2} \right) \]

\[ = \frac{\pi}{6} + 2 \left( -1 + \frac{\sqrt{3}}{2} \right) \]

\[ = \frac{\pi}{6} + 2 \left( -1 + \frac{\sqrt{3}}{2} \right) \]

\[ = \frac{\pi}{6} + 2 \left( -1 + \frac{\sqrt{3}}{2} \right) \]

\[ = \frac{\pi}{6} + 2 \left( -1 + \frac{\sqrt{3}}{2} \right) \]

\[ = \frac{\pi}{6} + 2 \left( -1 + \frac{\sqrt{3}}{2} \right) \]

\[ = \frac{\pi}{6} + 2 \left( -1 + \frac{\sqrt{3}}{2} \right) \]

\[ = \frac{\pi}{6} + 2 \left( -1 + \frac{\sqrt{3}}{2} \right) \]

\[ = \frac{\pi}{6} + 2 \left( -1 + \frac{\sqrt{3}}{2} \right) \]

\[ = \frac{\pi}{6} + 2 \left( -1 + \frac{\sqrt{3}}{2} \right) \]

\[ = \frac{\pi}{6} + 2 \left( -1 + \frac{\sqrt{3}}{2} \right) \]

\[ = \frac{\pi}{6} + 2 \left( -1 + \frac{\sqrt{3}}{2} \right) \]

\[ = \frac{\pi}{6} + 2 \left( -1 + \frac{\sqrt{3}}{2} \right) \]

\[ = \frac{\pi}{6} + 2 \left( -1 + \frac{\sqrt{3}}{2} \right) \]

\[ = \frac{\pi}{6} + 2 \left( -1 + \frac{\sqrt{3}}{2} \right) \]

\[ = \frac{\pi}{6} + 2 \left( -1 + \frac{\sqrt{3}}{2} \right) \]

\[ = \frac{\pi}{6} + 2 \left( -1 + \frac{\sqrt{3}}{2} \right) \]

\[ = \frac{\pi}{6} + 2 \left( -1 + \frac{\sqrt{3}}{2} \right) \]

\[ = \frac{\pi}{6} + 2 \left( -1 + \frac{\sqrt{3}}{2} \right) \]

\[ = \frac{\pi}{6} + 2 \left( -1 + \frac{\sqrt{3}}{2} \right) \]

\[ = \frac{\pi}{6} + 2 \left( -1 + \frac{\sqrt{3}}{2} \right) \]

\[ = \frac{\pi}{6} + 2 \left( -1 + \frac{\sqrt{3}}{2} \right) \]

\[ = \frac{\pi}{6} + 2 \left( -1 + \frac{\sqrt{3}}{2} \right) \]

\[ = \frac{\pi}{6} + 2 \left( -1 + \frac{\sqrt{3}}{2} \right) \]

\[ = \frac{\pi}{6} + 2 \left( -1 + \frac{\sqrt{3}}{2} \right) \]

\[ = \frac{\pi}{6} + 2 \left( -1 + \frac{\sqrt{3}}{2} \right) \]

\[ = \frac{\pi}{6} + 2 \left( -1 + \frac{\sqrt{3}}{2} \right) \]

\[ = \frac{\pi}{6} + 2 \left( -1 + \frac{\sqrt{3}}{2} \right) \]

\[ = \frac{\pi}{6} + 2 \left( -1 + \frac{\sqrt{3}}{2} \right) \]

\[ = \frac{\pi}{6} + 2 \left( -1 + \frac{\sqrt{3}}{2} \right) \]

\[ = \frac{\pi}{6} + 2 \left( -1 + \frac{\sqrt{3}}{2} \right) \]

\[ = \frac{\pi}{6} + 2 \left( -1 + \frac{\sqrt{3}}{2} \right) \]

\[ = \frac{\pi}{6} + 2 \left( -1 + \frac{\sqrt{3}}{2} \right) \]

\[ = \frac{\pi}{6} + 2 \left( -1 + \frac{\sqrt{3}}{2} \right) \]

\[ = \frac{\pi}{6} + 2 \left( -1 + \frac{\sqrt{3}}{2} \right) \]

\[ = \frac{\pi}{6} + 2 \left( -1 + \frac{\sqrt{3}}{2} \right) \]

\[ = \frac{\pi}{6} + 2 \left( -1 + \frac{\sqrt{3}}{2} \right) \]

\[ = \frac{\pi}{6} + 2 \left( -1 + \frac{\sqrt{3}}{2} \right) \]

\[ = \frac{\pi}{6} + 2 \left( -1 + \frac{\sqrt{3}}{2} \right) \]

\[ = \frac{\pi}{6} + 2 \left( -1 + \frac{\sqrt{3}}{2} \right) \]

\[ = \frac{\pi}{6} + 2 \left( -1 + \frac{\sqrt{3}}{2} \right) \]

\[ = \frac{\pi}{6} + 2 \left( -1 + \frac{\sqrt{3}}{2} \right) \]

\[ = \frac{\pi}{6} + 2 \left( -1 + \frac{\sqrt{3}}{2} \right) \]

\[ = \frac{\pi}{6} + 2 \left( -1 + \frac{\sqrt{3}}{2} \right) \]

\[ = \frac{\pi}{6} + 2 \left( -1 + \frac{\sqrt{3}}{2} \right) \]

\[ = \frac{\pi}{6} + 2 \left( -1 + \frac{\sqrt{3}}{2} \right) \]

\[ = \frac{\pi}{6} + 2 \left( -1 + \frac{\sqrt{3}}{2} \right) \]

\[ = \frac{\pi}{6} + 2 \left( -1 + \frac{\sqrt{3}}{2} \right) \]

\[ = \frac{\pi}{6} + 2 \left( -1 + \frac{\sqrt{3}}{2} \right) \]

\[ = \frac{\pi}{6} + 2 \left( -1 + \frac{\sqrt{3}}{2} \right) \]

\[ = \frac{\pi}{6} + 2 \left( -1 + \frac{\sqrt{3}}{2} \right) \]

\[ = \frac{\pi}{6} + 2 \left( -1 + \frac{\sqrt{3}}{2} \right) \]

\[ = \frac{\pi}{6} + 2 \left( -1 + \frac{\sqrt{3}}{2} \right) \]

\[ = \frac{\pi}{6} + 2 \left( -1 + \frac{\sqrt{3}}{2} \right) \]

\[ = \frac{\pi}{6} + 2 \left( -1 + \frac{\sqrt{3}}{2} \right) \]

\[ = \frac{\pi}{6} + 2 \left( -1 + \frac{\sqrt{3}}{2} \right) \]

\[ = \frac{\pi}{6} + 2 \left( -1 + \frac{\sqrt{3}}{2} \right) \]

\[ = \frac{\pi}{6} + 2 \left( -1 + \frac{\sqrt{3}}{2} \right) \]

\[ = \frac{\pi}{6} + 2 \left( -1 + \frac{\sqrt{3}}{2} \right) \]

\[ = \frac{\pi}{6} + 2 \left( -1 + \frac{\sqrt{3}}{2} \right) \]

\[ = \frac{\pi}{6} + 2 \left( -1 + \frac{\sqrt{3}}{2} \right) \]

\[ = \frac{\pi}{6} + 2 \left( -1 + \frac{\sqrt{3}}{2} \right) \]

\[ = \frac{\pi}{6} + 2 \left( -1 + \frac{\sqrt{3}}{2} \right) \]

\[ = \frac{\pi}{6} + 2 \left( -1 + \frac{\sqrt{3}}{2} \right) \]

\[ = \frac{\pi}{6} + 2 \left( -1 + \frac{\sqrt{3}}{2} \right) \]

\[ = \frac{\pi}{6} + 2 \left( -1 + \frac{\sqrt{3}}{2} \right) \]

\[ = \frac{\pi}{6} + 2 \left( -1 + \frac{\sqrt{3}}{2} \right) \]

\[ = \frac{\pi}{6} + 2 \left( -1 + \frac{\sqrt{3}}{2} \right) \]

\[ = \frac{\pi}{6} + 2 \left( -1 + \frac{\sqrt{3}}{2} \right) \]

\[ = \frac{\pi}{6} + 2 \left( -1 + \frac{\sqrt{3}}{2} \right) \]

\[ = \frac{\pi}{6} + 2 \left( -1 + \frac{\sqrt{3}}{2} \right) \]

\[ = \frac{\pi}{6} + 2 \left( -1 + \frac{\sqrt{3}}{2} \right) \]

\[ = \frac{\pi}{6} + 2 \left( -1 + \frac{\sqrt{3}}{2} \right) \]

\[ = \frac{\pi}{6} + 2 \left( -1 + \frac{\sqrt{3}}{2} \right) \]

\[ = \frac{\pi}{6} + 2 \left( -1 + \frac{\sqrt{3}}{2} \right) \]

\[ = \frac{\pi}{6} + 2 \left( -1 + \frac{\sqrt{3}}{2} \right) \]

\[ = \frac{\pi}{6} + 2 \left( -1 + \frac{\sqrt{3}}{2} \right) \]

\[ = \frac{\pi}{6} + 2 \left( -1 + \frac{\sqrt{3}}{2} \right) \]

\[ = \frac{\pi}{6} + 2 \left( -1 + \frac{\sqrt{3}}{2} \right) \]

\[ = \frac{\pi}{6} + 2 \left( -1 + \frac{\sqrt{3}}{2} \right) \]

\[ = \frac{\pi}{6} + 2 \left( -1 + \frac{\sqrt{3}}{2} \right) \]

\[ = \frac{\pi}{6} + 2 \left( -1 + \frac{\sqrt{3}}{2} \right) \]

\[ = \frac{\pi}{6} + 2 \left( -1 + \frac{\sqrt{3}}{2} \right) \]

\[ = \frac{\pi}{6} + 2 \left( -1 + \frac{\sqrt{3}}{2} \right) \]

\[ = \frac{\pi}{6} + 2 \left( -1 + \frac{\sqrt{3}}{2} \right) \]

\[ = \frac{\pi}{6} + 2 \left( -1 + \frac{\sqrt{3}}{2} \right) \]

\[ = \frac{\pi}{6} + 2 \left( -1 + \frac{\sqrt{3}}{2} \right) \]

\[ = \frac{\pi}{6} + 2 \left( -1 + \frac{\sqrt{3}}{2} \right) \]

\[ = \frac{\pi}{6} + 2 \left( -1 + \frac{\sqrt{3}}{2} \right) \]

\[ = \frac{\pi}{6} + 2 \left( -1 + \frac{\sqrt{3}}{2} \right) \]

\[ = \frac{\pi}{6} + 2 \left( -1 + \frac{\sqrt{3}}{2} \right) \]

\[ = \frac{\pi}{6} + 2 \left( -1 + \frac{\sqrt{3}}{2} \right) \]

\[ = \frac{\pi}{6} + 2 \left( -1 + \frac{\sqrt{3}}{2} \right) \]

\[ = \frac{\pi}{6} + 2 \left( -1 + \frac{\sqrt{3}}{2} \right) \]

\[ = \frac{\pi}{6} + 2 \left( -1 + \frac{\sqrt{3}}{2} \right) \]

\[ = \frac{\pi}{6} + 2 \left( -1 + \frac{\sqrt{3}}{2} \right) \]

\[ = \frac{\pi}{6} + 2 \left( -1 + \frac{\sqrt{3}}{2} \right) \]

\[ = \frac{\pi}{6} + 2 \left( -1 + \frac{\sqrt{3}}{2} \right) \]

\[ = \frac{\pi}{6} + 2 \left( -1 + \frac{\sqrt{3}}{2} \right) \]

\[ = \frac{\pi}{6} + 2 \left( -1 + \frac{\sqrt{3}}{2} \right) \]

\[ = \frac{\pi}{6} + 2 \left( -1 + \frac{\sqrt{3}}{2} \right) \]

\[ = \frac{\pi}{6} + 2 \left( -1 + \frac{\sqrt{3}}{2} \right) \]

\[ = \frac{\pi}{6} + 2 \left( -1 + \frac{\sqrt{3}}{2} \right) \]

\[ = \frac{\pi}{6} + 2 \left( -1 + \frac{\sqrt{3}}{2} \right) \]

\[ = \frac{\pi}{6} + 2 \left( -1 + \frac{\sqrt{3}}{2} \right) \]

\[ = \frac{\pi}{6} + 2 \left( -1 + \frac{\sqrt{3}}{2} \right) \]

\[ = \frac{\pi}{6} + 2 \left( -1 + \frac{\sqrt{3}}{2} \right) \]

\[ = \frac{\pi}{6} + 2 \left( -1 + \frac{\sqrt{3}}{2} \right) \]

\[ = \frac{\pi}{6} + 2 \left( -1 + \frac{\sqrt{3}}{2} \right) \]

\[ = \frac{\pi}{6} + 2 \left( -1 + \frac{\sqrt{3}}{2} \right) \]

\[ = \frac{\pi}{6} + 2 \left( -1 + \frac{\sqrt{3}}{2} \right) \]

\[ = \frac{\pi}{6} + 2 \left( -1 + \frac{\sqrt{3}}{2} \right) \]

\[ = \frac{\pi}{6} + 2 \left( -1 + \frac{\sqrt{3}}{2} \right) \]

\[ = \frac{\pi}{6} + 2 \left( -1 + \frac{\sqrt{3}}{2} \right) \]

\[ = \frac{\pi}{6} + 2 \left( -1 + \frac{\sqrt{3}}{2} \right) \]

\[ = \frac{\pi}{6} + 2 \left( -1 + \frac{\sqrt{3}}{2} \right) \]

\[ = \frac{\pi}{6} + 2 \left( -1 + \frac{\sqrt{3}}{2} \right) \]

\[ = \frac{\pi}{6} + 2 \left( -1 + \frac{\sqrt{3}}{2} \right) \]

\[ = \frac{\pi}{6} + 2 \left( -1 + \frac{\sqrt{3}}{2} \right) \]

\[ = \frac{\pi}{6} + 2 \left( -1 + \frac{\sqrt{3}}{2} \right) \]

\[ = \frac{\pi}{6} + 2 \left( -1 + \frac{\sqrt{3}}{2} \right) \]

\[ = \frac{\pi}{6} + 2 \left( -1 + \frac{\sqrt{3}}{2} \right) \]

\[ = \frac{\pi}{6} + 2 \left( -1 + \frac{\sqrt{3}}{2} \right) \]

\[ = \frac{\pi}{6} + 2 \left( -1 + \frac{\sqrt{3}}{2} \right) \]

\[ = \frac{\pi}{6} + 2 \left( -1 + \frac{\sqrt{3}}{2} \right) \]

\[ = \frac{\pi}{6} + 2 \left( -1 + \frac{\sqrt{3}}{2} \right) \]

\[ = \frac{\pi}{6} + 2 \left( -1 + \frac{\sqrt{3}}{2} \right) \]

\[ = \frac{\pi}{6} + 2 \left( -1 + \frac{\sqrt{3}}{2} \right) \]

\[ = \frac{\pi}{6} + 2 \left( -1 + \frac{\sqrt{3}}{2} \right) \]

\[ = \frac{\pi}{6} + 2 \left( -1 + \frac{\sqrt{3}}{2} \right) \]

\[ = \frac{\pi}{6} + 2 \left( -1 + \frac{\sqrt{3}}{2} \right) \]

\[ = \frac{\pi}{6} + 2 \left( -1 + \frac{\sqrt{3}}{2} \right) \]

\[ = \frac{\pi}{6} + 2 \left( -1 + \frac{\sqrt{3}}{2} \right) \]

\[ = \frac{\pi}{6} + 2 \left( -1 + \frac{\sqrt{3}}{2} \right) \]

\[ = \frac{\pi}{6} + 2 \left( -1 + \frac{\sqrt{3}}{2} \right) \]

\[ = \frac{\pi}{6} + 2 \left( -1 + \frac{\sqrt{3}}{2} \right) \]

\[ = \frac{\pi}{6} + 2 \left( -1 + \frac{\sqrt{3}}{2} \right) \]

\[ = \frac{\pi}{6} + 2 \left( -1 + \frac{\sqrt{3}}{2} \right) \]

\[ = \frac{\pi}{6} + 2 \left( -1 + \frac{\sqrt{3}}{2} \right) \]

\[ = \frac{\pi}{6} + 2 \left( -1 + \frac{\sqrt{3}}{2} \right) \]

\[ = \frac{\pi}{6} + 2 \left( -1 + \frac{\sqrt{3}}{2} \right) \]

\[ = \frac{\pi}{6} + 2 \left( -1 + \frac{\sqrt{3}}{2} \right) \]

\[ = \frac{\pi}{6} + 2 \left( -1 + \frac{\sqrt{3}}{2} \right) \]

\[ = \frac{\pi}{6} + 2 \left( -1 + \frac{\sqrt{3}}{2} \right) \]

\[ = \frac{\pi}{6} + 2 \left( -1 + \frac{\sqrt{3}}{2} \right) \]

\[ = \frac{\pi}{6} + 2 \left( -1 + \frac{\sqrt{3}}{2} \right) \]

\[ = \frac{\pi}{6} + 2 \left( -1 + \frac{\sqrt{3}}{2} \right) \]

\[ = \frac{\pi}{6} + 2 \left( -1 + \frac{\sqrt{3}}{2} \right) \]

\[ = \frac{\pi}{6} + 2 \left( -1 + \frac{\sqrt{3}}{2} \right) \]

\[ = \frac{\pi}{6} + 2 \left( -1 + \frac{\sqrt{3}}{2} \right) \]

\[ = \frac{\pi}{6} + 2 \left( -1 + \frac{\sqrt{3}}{2} \right) \]

\[ = \