
To solve the definite integral \(\int_0^1 \arccos(x) J_1(2x) \, dx\), we proceed with integration by parts and utilize properties of Bessel functions.

### Step 1: Integration by Parts
Let \(u = \arccos(x)\) and \(dv = J_1(2x) \, dx\). Then:
- \(du = -\frac{1}{\sqrt{1 - x^2}} \, dx\)
- \(v = -\frac{1}{2} J_0(2x)\) (since \(\int J_1(az) \, dz = -\frac{1}{a} J_0(az) + C\) with \(a=2\))

By integration by parts:
\[
\int_0^1 \arccos(x) J_1(2x) \, dx = \left[ uv \right]_0^1 - \int_0^1 v \, du
\]

### Step 2: Evaluate Boundary Term \(\left[ uv \right]_0^1\)
- At \(x=1\): \(\arccos(1) = 0\), so \(uv = 0\).
- At \(x=0\): \(\arccos(0) = \frac{\pi}{2}\) and \(v(0) = -\frac{1}{2} J_0(0) = -\frac{1}{2}\) (since \(J_0(0) = 1\)). Thus, \(uv = \frac{\pi}{2} \cdot \left(-\frac{1}{2}\right) = -\frac{\pi}{4}\).

Thus:
\[
\left[ uv \right]_0^1 = 0 - \left(-\frac{\pi}{4}\right) = \frac{\pi}{4}
\]

### Step 3: Evaluate Remaining Integral \(-\int_0^1 v \, du\)
Substituting \(v = -\frac{1}{2} J_0(2x)\) and \(du = -\frac{1}{\sqrt{1 - x^2}} \, dx\):
\[
-\int_0^1 v \, du = -\int_0^1 \left(-\frac{1}{2} J_0(2x)\right) \left(-\frac{1}{\sqrt{1 - x^2}}\right) dx = -\frac{1}{2} \int_0^1 \frac{J_0(2x)}{\sqrt{1 - x^2}} \, dx
\]

### Step 4: Simplify the Integral \(\int_0^1 \frac{J_0(2x)}{\sqrt{1 - x^2}} \, dx\)
Using the substitution \(x = \sin\theta\) (so \(dx = \cos\theta \, d\theta\) and \(\sqrt{1 - x^2} = \cos\theta\)), the integral becomes:
\[
\int_0^{\pi/2} J_0(2 \sin\theta) \, d\theta
\]

### Step 5: Use Bessel Function Identity
A key identity for Bessel functions states:
\[
\int_0^{\pi/2} J_0(2z \sin\theta) \, d\theta = \frac{\pi}{2} \left[ J_0(z) \right]^2
\]
For \(z = 1\), this gives:
\[
\int_0^{\pi/2} J_0(2 \sin\theta) \, d\theta = \frac{\pi}{2} \left[ J_0(1) \right]^2
\]

### Step 6: Combine Results
Substituting back, the original integral becomes:
\[
\int_0^1 \arccos(x) J_1(2x) \, dx = \frac{\pi}{4} - \frac{1}{2} \cdot \frac{\pi}{2} \left[ J_0(1) \right]^2 = \frac{\pi}{4} \left(1 - \left[ J_0(1) \right]^2 \right)
\]

### Numerical Approximation
Using \(J_0(1) \approx 0.7651976865579666\), we compute:
\[
\left[ J_0(1) \right]^2 \approx 0.5855272793
\]
Thus:
\[
\frac{\pi}{4} \left(1 - 0.5855272793\right) \approx \frac{\pi}{4} \cdot 0.4144727207 \approx 0.3256803685
\]

### Final Answer
{"answer": "\\frac{\\pi}{4} \\left(1 - J_0(1)^2\\right)", "numerical_answer": "0.3256803685"}