Let’s compute the integral:

\[
I = \int_{0}^{7}\left(\sqrt[3]{\sqrt{x^{2}+1}+x}-\sqrt[3]{\sqrt{x^{2}+1}-x}\right)\:\mathrm{d}x.
\]

**Step 1: Substitution**

Let’s try the substitution:
Let \( u = \sqrt{x^2 + 1} + x \).

Then,
\( \sqrt{x^2 + 1} = u - x \)

Square both sides:
\[
x^2 + 1 = (u - x)^2 \implies u^2 - 2ux + x^2 = x^2 + 1
\]
\[
u^2 - 2ux = 1
\]
\[
u^2 - 1 = 2ux \implies x = \frac{u^2 - 1}{2u}
\]

Now return to the limits:
When \( x = 0 \): \( u = \sqrt{0^2 + 1} + 0 = 1 \)
When \( x = 7 \): \( u = \sqrt{49 + 1} + 7 = \sqrt{50} + 7 = 5\sqrt{2} + 7 \)

Now, we compute \( \sqrt[3]{\sqrt{x^2+1}+x} = u^{1/3} \).
Now, \( \sqrt[3]{\sqrt{x^2+1}-x} = (\sqrt{x^2+1} - x)^{1/3} \).

But \(\sqrt{x^2+1} - x = \frac{1}{u - x} = \frac{1}{u} - x\), but to find a relationship:

Let’s try to rationalize or manipulate the expression.

Alternative: Consider the following algebraic manipulations.

Let’s try substitution \( x = \sinh t \).
Then \( dx = \cosh t \, dt \), and \( \sqrt{x^2 + 1} = \sqrt{\sinh^2 t + 1} = \cosh t \).

So

\[
\sqrt[3]{\sqrt{x^2+1} + x} = \sqrt[3]{\cosh t + \sinh t} = \sqrt[3]{e^t}
\]
because \( \cosh t + \sinh t = e^t \).

Similarly,

\[
\sqrt[3]{\sqrt{x^2+1} - x} = \sqrt[3]{\cosh t - \sinh t} = \sqrt[3]{e^{-t}}
\]

Therefore,
\[
\sqrt[3]{\sqrt{x^2+1} + x} - \sqrt[3]{\sqrt{x^2+1} - x} = e^{t/3} - e^{-t/3}
\]

Now, compute the transformed limits:

When \( x = 0 \): \( \sinh t = 0 \implies t = 0 \)
When \( x = 7 \): \( t_1 = \sinh^{-1}(7) \)

So our integral becomes:
\[
I = \int_{x=0}^{x=7} \left(\sqrt[3]{\sqrt{x^{2}+1}+x}-\sqrt[3]{\sqrt{x^{2}+1}-x}\right)\:\mathrm{d}x 
= \int_{t = 0}^{t = \sinh^{-1}(7)} \left(e^{t/3} - e^{-t/3}\right) \cosh t \; dt
\]

**Step 2: Expand and Integrate**

Let’s expand:
\[
\int \left(e^{t/3} - e^{-t/3}\right) \cosh t \; dt = \int e^{t/3} \cosh t \; dt - \int e^{-t/3} \cosh t \; dt
\]

Let’s compute \( \int e^{\alpha t} \cosh t \, dt \).

Recall:

\( \cosh t = \frac{e^{t} + e^{-t}}{2} \), so

\[
e^{\alpha t} \cosh t = \frac{1}{2}(e^{(\alpha+1)t} + e^{(\alpha-1)t})
\]

Therefore,

\[
\int e^{\alpha t} \cosh t \, dt = \frac{1}{2} \int e^{(\alpha+1)t} dt + \frac{1}{2} \int e^{(\alpha-1)t} dt = \frac{1}{2} \left( \frac{e^{(\alpha+1)t}}{\alpha+1} + \frac{e^{(\alpha-1)t}}{\alpha-1} \right )
\]

Back to our case:

- For \( e^{t/3} \cosh t \), \( \alpha = 1/3 \):

\[
\int e^{t/3} \cosh t \, dt = \frac{1}{2} \left( \frac{e^{(1/3+1)t}}{1/3+1} + \frac{e^{(1/3-1)t}}{1/3-1} \right)
= \frac{1}{2} \left( \frac{e^{(4/3)t}}{4/3} + \frac{e^{(-2/3)t}}{-2/3} \right)
\]

Similarly,

- For \( e^{-t/3} \cosh t \), \( \alpha = -1/3 \):

\[
\int e^{-t/3} \cosh t \, dt = \frac{1}{2} \left( \frac{e^{(2/3)t}}{2/3} + \frac{e^{-(4/3)t}}{-4/3} \right)
\]

So the difference:

\[
I = \left[ \int e^{t/3}\cosh t \;dt - \int e^{-t/3}\cosh t \;dt \right]_{t=0}^{t_1}
\]

Let’s write these results:

\[
\int e^{t/3}\cosh t \, dt = \frac{3}{8} e^{(4/3)t} - \frac{3}{4} e^{(-2/3)t}
\]
\[
\int e^{-t/3}\cosh t \, dt = \frac{3}{4} e^{(2/3)t} - \frac{3}{8} e^{(-4/3)t}
\]

(Verifying: \(1/(4/3) = 3/4\), \(1/(-2/3) = -3/2\), but with the factor \(1/2\) in front, so \((1/2)\cdot(-3/2) = -3/4\). Confirmed.)

So,
\[
I = \left[ \frac{3}{8} e^{(4/3)t} - \frac{3}{4}e^{(-2/3)t} - \left(\frac{3}{4}e^{(2/3)t} - \frac{3}{8}e^{(-4/3)t}\right) \right]_{t=0}^{t_1}
\]
\[
I = \left[ \frac{3}{8} e^{(4/3)t} - \frac{3}{4}e^{(-2/3)t} - \frac{3}{4}e^{(2/3)t} + \frac{3}{8}e^{(-4/3)t} \right]_{t=0}^{t_1}
\]

Or, equivalent:

\[
I = \frac{3}{8} \Big[ e^{(4/3)t} + e^{-(4/3)t} \Big] - \frac{3}{4} \Big[ e^{(2/3)t} + e^{-(2/3)t} \Big ] \Bigg|_{t=0}^{t_1}
\]

Let’s write this as:

\[
I = \left\{ \frac{3}{8}\Big( e^{4t/3} + e^{-4t/3} \Big) - \frac{3}{4}\Big( e^{2t/3} + e^{-2t/3} \Big) \right\}_{t=0}^{t_1}
\]

Therefore, the exact answer is:

\[
I = \left[ \frac{3}{8}\left( e^{4t/3} + e^{-4t/3} \right) - \frac{3}{4}\left( e^{2t/3} + e^{-2t/3} \right) \right ]_{t=0}^{t_1}
\]

Recall \( t_1 = \sinh^{-1}(7) \).

So,

\[
I = \left\{ \frac{3}{8}\left[ e^{4\sinh^{-1}(7)/3} + e^{-4\sinh^{-1}(7)/3} \right] - \frac{3}{4}\left[ e^{2\sinh^{-1}(7)/3} + e^{-2\sinh^{-1}(7)/3} \right] \right\} \\
- \left( \frac{3}{8}\left[ e^{0}+e^{0} \right] - \frac{3}{4}[e^0+e^0] \right )
\]

\[
e^{0}+e^{0} = 2
\]

So at \( t=0 \):

\[
\frac{3}{8}\cdot 2 - \frac{3}{4} \cdot 2 = \frac{3}{4} - \frac{3}{2} = -\frac{3}{4}
\]

So the definite value:

\[
I = \left\{ \frac{3}{8}\left[ e^{4\sinh^{-1}(7)/3} + e^{-4\sinh^{-1}(7)/3} \right] - \frac{3}{4}\left[ e^{2\sinh^{-1}(7)/3} + e^{-2\sinh^{-1}(7)/3} \right] + \frac{3}{4} \right\}
\]

**Step 3: Numerical approximation**

We need to calculate \( \sinh^{-1}(7) \):

\[
\sinh^{-1}(x) = \ln(x+\sqrt{x^2+1}) \implies \sinh^{-1}(7) = \ln(7+\sqrt{49+1}) = \ln(7+7.071067812)
\]
\[
= \ln(14.071067812) \approx 2.6441207611
\]

Now compute the exponentials:

- \( 4t/3 \approx 4 \cdot 2.6441207611 / 3 = 3.5254943481 \)
- \( 2t/3 \approx 2 \cdot 2.6441207611 / 3 = 1.7627471740 \)

- \( e^{3.5254943481} \approx 33.9879358191 \)
- \( e^{-3.5254943481} \approx 0.0287367428 \)
- \( e^{1.7627471740} \approx 5.8301270204 \)
- \( e^{-1.7627471740} \approx 0.1721818754 \)

So,

\[
I \approx \frac{3}{8}(33.9879358191 + 0.0287367428) - \frac{3}{4}(5.8301270204 + 0.1721818754) + \frac{3}{4}
\]

Calculate:

- \( 33.9879358191 + 0.0287367428 = 34.0166725619 \)
- \( 5.8301270204 + 0.1721818754 = 6.0023088958 \)

Plug in:

- \( \frac{3}{8} \cdot 34.0166725619 = 12.7562522107 \)
- \( \frac{3}{4} \cdot 6.0023088958 = 4.5017316719 \)
- \( + \frac{3}{4} = 0.75 \)

Therefore

\[
I \approx 12.7562522107 - 4.5017316719 + 0.75 = (12.7562522107 - 4.5017316719) + 0.75 = 8.2545205388 + 0.75 = \boxed{9.0045205388}
\]

So to 10 decimal places:
\[
I \approx 9.0045205388
\]

**Step 4: JSON output**

```json
{"answer": "\\frac{3}{8}\\left(e^{\\frac{4}{3}\\sinh^{-1}(7)} + e^{-\\frac{4}{3}\\sinh^{-1}(7)}\\right) - \\frac{3}{4}\\left(e^{\\frac{2}{3}\\sinh^{-1}(7)} + e^{-\\frac{2}{3}\\sinh^{-1}(7)}\\right) + \\frac{3}{4}", "numerical_answer": "9.0045205388"}
```