Let
\[
I = \int_{0}^{7}\left(\sqrt[3]{\sqrt{x^{2}+1}+x}-\sqrt[3]{\sqrt{x^{2}+1}-x}\right) dx
\]

Let’s denote:
\[
f(x) = \sqrt[3]{\sqrt{x^{2}+1}+x}-\sqrt[3]{\sqrt{x^{2}+1}-x}
\]

Let’s attempt a substitution to simplify this expression. 

Let’s try and find the antiderivative analytically.

### Step 1: Guess the Right Substitution

Let’s try to write \( f(x) \) in terms of a single variable. 

Let’s try \( x = \sinh t \). Then, \( dx = \cosh t \, dt \), and \( \sqrt{x^2 + 1} = \cosh t \):

- \( \sqrt{x^2 + 1} = \sqrt{\sinh^2 t + 1} = \sqrt{\cosh^2 t} = \cosh t \)
- \( x = \sinh t \)

So,
\[
\sqrt[3]{\sqrt{x^2 + 1} + x} = \sqrt[3]{\cosh t + \sinh t}
\]
\[
\sqrt[3]{\sqrt{x^2 + 1} - x} = \sqrt[3]{\cosh t - \sinh t}
\]

But,
\[
\cosh t \pm \sinh t = e^{\pm t}
\]
Thus,
\[
f(x) = \sqrt[3]{e^t} - \sqrt[3]{e^{-t}} = e^{t/3} - e^{-t/3}
= 2 \sinh \left( \frac{t}{3} \right)
\]

Recall,
- When \( x = 0 \), \( \sinh t = 0 \implies t = 0 \)
- When \( x = 7 \), \( \sinh t = 7 \implies t = \sinh^{-1} 7 \)

Thus the bounds are \( t = 0 \) to \( t = \sinh^{-1} 7 \). Also, for this substitution, \( dx = \cosh t dt \).

So,
\[
I = \int_{x=0}^{x=7} f(x) dx = \int_{t=0}^{t=\sinh^{-1} 7} 2\sinh\left(\frac{t}{3}\right) \cosh t \, dt
\]

### Step 2: Integrate

Let’s expand:
\[
I = 2 \int_{0}^{\sinh^{-1} 7} \sinh\left(\frac{t}{3}\right) \cosh t \, dt
\]

We can write:
\[
\sinh\left(\frac{t}{3}\right)\cosh t = \frac{1}{2}\left(e^{t/3} - e^{-t/3}\right) \cdot \frac{1}{2}\left(e^t + e^{-t}\right)
\]
Let’s multiply:
\[
= \frac{1}{4} \left( e^{t/3} e^{t} + e^{t/3} e^{-t} - e^{-t/3} e^{t} - e^{-t/3} e^{-t} \right)
= \frac{1}{4} \left( e^{t(1 + 1/3)} + e^{t/3 - t} - e^{-t/3 + t} - e^{-t(1 + 1/3)} \right)
\]
\[
1 + 1/3 = 4/3
\]
So,
\[
= \frac{1}{4} \left( e^{4t/3} + e^{-2t/3} - e^{2t/3} - e^{-4t/3} \right)
\]
So the full integral is:
\[
I = 2 \int_{0}^{\sinh^{-1} 7} \frac{1}{4} \left( e^{4t/3} + e^{-2t/3} - e^{2t/3} - e^{-4t/3} \right) \, dt
\]
\[
= \frac{1}{2} \int_{0}^{\sinh^{-1} 7} \left( e^{4t/3} + e^{-2t/3} - e^{2t/3} - e^{-4t/3} \right) dt
\]

Compute each term:

The antiderivative of \( e^{kt} \) is \( (1/k)e^{kt} \):

- \( \int e^{4t/3} dt = \frac{3}{4} e^{4t/3} \)
- \( \int e^{-2t/3} dt = -\frac{3}{2} e^{-2t/3} \)
- \( \int e^{2t/3} dt = \frac{3}{2} e^{2t/3} \)
- \( \int e^{-4t/3} dt = -\frac{3}{4} e^{-4t/3} \)

Therefore,
\[
I = \frac{1}{2} \left[
\frac{3}{4} e^{4t/3}
- \frac{3}{2} e^{-2t/3}
- \frac{3}{2} e^{2t/3}
+ \frac{3}{4} e^{-4t/3}
\right]_{t=0}^{t=\sinh^{-1} 7}
\]
(Negative signs checked; yes, the minus sign is correctly taken, e.g., \(-e^{-4t/3} \to +\frac{3}{4}e^{-4t/3}\) after integrating.)

So, simplify:
\[
I = \frac{3}{8}
\left[
e^{4t/3} + e^{-4t/3}
- 2 e^{2t/3}
- 2 e^{-2t/3}
\right]_{t=0}^{t=\sinh^{-1} 7}
\]

In other words,
\[
I = \frac{3}{8}
\left\{
\left(
e^{4t/3} + e^{-4t/3}
- 2 e^{2t/3}
- 2 e^{-2t/3}
\right)
\Bigg|_{t=0}^{t=\sinh^{-1} 7}
\right\}
\]

Let’s write the explicit expression:

Let \( T = \sinh^{-1} 7 \), then

\[
I = \frac{3}{8} \left[ ( e^{4T/3} + e^{-4T/3} - 2e^{2T/3} - 2e^{-2T/3}) - ( e^{0} + e^{0} - 2e^0 - 2e^0 ) \right]
\]
But \( e^0 = 1 \), so \( 1 + 1 - 2 - 2 = -2 \)

So,

\[
I = \frac{3}{8} \left( e^{4T/3} + e^{-4T/3} - 2e^{2T/3} - 2e^{-2T/3} + 2 \right)
\]

Or, to be explicit,
\[
I = \frac{3}{8} \left( e^{\frac{4}{3} \sinh^{-1} 7} + e^{-\frac{4}{3} \sinh^{-1} 7}
- 2 e^{\frac{2}{3} \sinh^{-1} 7}
- 2 e^{-\frac{2}{3} \sinh^{-1} 7}
+ 2
\right)
\]

### Step 3: Numeric Evaluation

First, compute \( T = \sinh^{-1} 7 \):

\[
\sinh^{-1} 7 = \ln\left( 7 + \sqrt{49 + 1} \right) = \ln(7 + \sqrt{50}) 
\]
\[
\sqrt{50} = 7.0710678118654755
\]
\[
7 + 7.0710678118654755 = 14.071067811865476
\]
\[
T = \ln(14.071067811865476) \approx 2.644120761058629
\]

Now,
- \( \frac{2}{3}T = 2/3 \cdot 2.644120761058629 = 1.762747174039086 \)
- \( \frac{4}{3}T = 2 \cdot 1.762747174039086 = 3.525494348078172 \)

Now compute exponentials:

- \( e^{3.525494348078172} = \exp(3.525494348078172) = 33.99258647526313 \)
- \( e^{-3.525494348078172} = 1/33.99258647526313 = 0.02941437496693412 \)
- \( e^{1.762747174039086} = \exp(1.762747174039086) = 5.829741880085565 \)
- \( e^{-1.762747174039086} = 1/5.829741880085565 = 0.1715264130430672 \)

Plug in:
\[
I = \frac{3}{8}\left(33.99258647526313 + 0.02941437496693412 - 2\times 5.829741880085565 - 2\times 0.1715264130430672 + 2 \right)
\]

Evaluate terms:

- \( 33.99258647526313 + 0.02941437496693412 = 34.02200085023007 \)
- \( 2 \times 5.829741880085565 = 11.65948376017113 \)
- \( 2 \times 0.1715264130430672 = 0.3430528260861344 \)
- \( -11.65948376017113 - 0.3430528260861344 = -12.002536586257267 \)
- \( 34.02200085023007 - 12.002536586257267 = 22.0194642639728 \)
- \( 22.0194642639728 + 2 = 24.0194642639728 \)

So,

\[
I = \frac{3}{8} \times 24.0194642639728 = 0.375 \times 24.0194642639728 = 9.0072990989898
\]
So, rounded to 10 decimal places: \( 9.0072990990 \)

### Step 4: Final JSON Output

```json
{"answer": "\\frac{3}{8}\\left(e^{\\frac{4}{3}\\sinh^{-1} 7}+e^{-\\frac{4}{3}\\sinh^{-1} 7}-2e^{\\frac{2}{3}\\sinh^{-1} 7}-2e^{-\\frac{2}{3}\\sinh^{-1} 7}+2\\right)", "numerical_answer": "9.0072990990"}
```