Let's evaluate the integral:
\[
I = \int_0^\infty \frac{\tanh(x)}{e^x} dx
\]

---

### Step 1: Analytical Calculation

First, write \(\tanh(x)\) as:
\[
\tanh(x) = \frac{e^x - e^{-x}}{e^x + e^{-x}}
\]
So,
\[
\frac{\tanh(x)}{e^x} = \frac{e^x - e^{-x}}{e^x + e^{-x}} \cdot \frac{1}{e^x}
= \frac{e^x - e^{-x}}{e^{2x} + 1}
\]

Let’s see this clearly:
\[
e^x + e^{-x} = \frac{e^{2x} + 1}{e^x}
\implies \tanh(x) = \frac{e^x - e^{-x}}{e^x + e^{-x}} = \frac{e^{2x} - 1}{e^{2x} + 1}
\]
Therefore,
\[
\frac{\tanh(x)}{e^x} = \frac{e^{2x}-1}{e^{2x}+1} \frac{1}{e^x} = \frac{e^x - e^{-x}}{e^{2x} + 1}
\]

So the integral becomes:
\[
I = \int_0^\infty \frac{e^x - e^{-x}}{e^{2x} + 1} dx
\]
\[
= \int_0^\infty \frac{e^x}{e^{2x}+1} dx - \int_0^\infty \frac{e^{-x}}{e^{2x}+1} dx
\]
Let’s call these \(I_1\) and \(I_2\), so \(I = I_1 - I_2\).

#### Evaluate \(I_1 = \int_0^\infty \frac{e^x}{e^{2x}+1} dx\)

Let \(u = e^x\), \(du = e^x dx\), so \(dx = du/u\).
As \(x \to 0\), \(u \to 1\), as \(x \to \infty\), \(u \to \infty\).

\[
I_1 = \int_{x=0}^{x \to \infty} \frac{e^x}{e^{2x}+1} dx = \int_{u=1}^{u \to \infty} \frac{u}{u^2+1} \cdot \frac{du}{u} = \int_1^\infty \frac{du}{u^2+1}
\]

This can be directly integrated:

\[
I_1 = \left.\arctan(u)\right|_{1}^{\infty} = \left(\frac{\pi}{2} - \frac{\pi}{4}\right) = \frac{\pi}{4}
\]

#### Evaluate \(I_2 = \int_0^\infty \frac{e^{-x}}{e^{2x}+1} dx\)

Let’s substitute \(x \to t\):

First, write \(e^{-x} = 1 / e^x\).
So,

\[
I_2 = \int_0^\infty \frac{1}{e^x (e^{2x}+1)} dx
\]

But \(e^{2x} + 1 = (e^x)^2 + 1\), so set \(u = e^x\), \(du = e^x dx\), \(dx = du/u\), when \(x=0, u=1\), \(x\to\infty, u\to\infty\):

\[
I_2 = \int_{x=0}^{\infty} \frac{1}{e^x (e^{2x}+1)} dx = \int_{u=1}^{\infty} \frac{1}{u (u^2+1)} \cdot \frac{du}{u}
= \int_1^{\infty} \frac{1}{u^2(u^2 + 1)} du
\]

Now decompose \(\frac{1}{u^2(u^2 + 1)}\):

Let’s use partial fractions:
\[
\frac{1}{u^2(u^2+1)} = \frac{A}{u} + \frac{B}{u^2} + \frac{C u + D}{u^2+1}
\]

Multiply both sides by \(u^2(u^2+1)\):

\[
1 = A u(u^2 + 1) + B(u^2 + 1) + (Cu + D) u^2
\]
\[
= A u^3 + A u + B u^2 + B + C u^3 + D u^2
\]
\[
= (A+C)u^3 + (B+D)u^2 + A u + B
\]

Set coefficients equal to zero:

Matching coefficients:
- \(u^3\): \(A + C = 0 \implies C = -A\)
- \(u^2\): \(B + D = 0 \implies D = -B\)
- \(u^1\): \(A\)
- constant: \(B\)

But actually, we are missing the terms -- let's correct the expansion.

Let me expand more directly:

\[
A/u + B/u^2 + (Cu + D)/(u^2+1) = \frac{A(u)(u^2+1) + B(u^2+1) + (Cu+D)u^2}{u^2(u^2+1)}
\]
\[
= \frac{A u^3 + A u + B u^2 + B + C u^3 + D u^2}{u^2(u^2+1)}
\]
\[
= \frac{(A+C)u^3 + (B + D)u^2 + A u + B}{u^2(u^2+1)}
\]
Set equal to numerator of original fraction:
\[
1 = (A+C)u^3 + (B+D)u^2 + A u + B 
\]
So, system:
- \(u^3:\) \(A + C = 0\)
- \(u^2:\) \(B + D = 0\)
- \(u^1:\) \(A = 0\)
- constant: \(B = 1\)

So \(A = 0\), \(B=1\), \(C = -A = 0\), \(D = -B = -1\).

So,
\[
\frac{1}{u^2(u^2+1)} = \frac{1}{u^2} - \frac{1}{u^2+1}
\]

Now integrate:
\[
I_2 = \int_1^{\infty} \left( \frac{1}{u^2} - \frac{1}{u^2+1} \right) du
\]

\[
= \left[ -\frac{1}{u} - \arctan(u) \right]_{u=1}^{u\to\infty}
\]

As \(u \to \infty\), \(-1/u \to 0\), \(\arctan(u) \to \pi/2\), at \(u=1\), \(-1/1 = -1\), \(\arctan(1) = \pi/4\):

So,
\[
I_2 = \left( 0 - \frac{\pi}{2} \right) - \left( -1 - \frac{\pi}{4} \right) = -\frac{\pi}{2} + 1 + \frac{\pi}{4} = 1 - \frac{\pi}{4}
\]

---

### Step 2: Combine Results

Recall,
\[
I = I_1 - I_2 = \frac{\pi}{4} - \left(1 - \frac{\pi}{4} \right) = \frac{\pi}{4} - 1 + \frac{\pi}{4} = \frac{\pi}{2} - 1
\]

---

### Step 3: Numerical Approximation

\[
\frac{\pi}{2} - 1 \approx \frac{3.1415926536}{2} - 1 \approx 1.5707963268 - 1 = 0.5707963268
\]

---

### Step 4: Output in JSON

```json
{"answer": "\\frac{\\pi}{2} - 1", "numerical_answer": "0.5707963268"}
```