To solve the definite integral \(\int_{0}^{1} \arcsin(x) \arccos(x) \, dx\), we will follow the steps outlined:

### Step 1: Analytical Computation

First, we use the identity \(\arcsin(x) + \arccos(x) = \frac{\pi}{2}\) for \(x \in [-1, 1]\). This allows us to rewrite the integrand:

\[
\arcsin(x) \arccos(x) = \arcsin(x) \left( \frac{\pi}{2} - \arcsin(x) \right) = \frac{\pi}{2} \arcsin(x) - \arcsin^2(x)
\]

Thus, the integral becomes:

\[
\int_{0}^{1} \arcsin(x) \arccos(x) \, dx = \int_{0}^{1} \left( \frac{\pi}{2} \arcsin(x) - \arcsin^2(x) \right) dx
\]

We can split this into two separate integrals:

\[
\int_{0}^{1} \arcsin(x) \arccos(x) \, dx = \frac{\pi}{2} \int_{0}^{1} \arcsin(x) \, dx - \int_{0}^{1} \arcsin^2(x) \, dx
\]

#### Integral 1: \(\int_{0}^{1} \arcsin(x) \, dx\)

To evaluate \(\int_{0}^{1} \arcsin(x) \, dx\), we use integration by parts. Let \(u = \arcsin(x)\) and \(dv = dx\). Then \(du = \frac{1}{\sqrt{1 - x^2}} dx\) and \(v = x\). Applying integration by parts:

\[
\int \arcsin(x) \, dx = x \arcsin(x) - \int \frac{x}{\sqrt{1 - x^2}} \, dx
\]

The remaining integral can be solved by substitution. Let \(t = 1 - x^2\), then \(dt = -2x \, dx\), so \(-\frac{1}{2} dt = x \, dx\):

\[
\int \frac{x}{\sqrt{1 - x^2}} \, dx = -\frac{1}{2} \int \frac{1}{\sqrt{t}} \, dt = -\sqrt{t} = -\sqrt{1 - x^2}
\]

Thus,

\[
\int \arcsin(x) \, dx = x \arcsin(x) + \sqrt{1 - x^2} + C
\]

Evaluating from 0 to 1:

\[
\int_{0}^{1} \arcsin(x) \, dx = \left[ x \arcsin(x) + \sqrt{1 - x^2} \right]_{0}^{1} = \left( 1 \cdot \frac{\pi}{2} + 0 \right) - \left( 0 + 1 \right) = \frac{\pi}{2} - 1
\]

#### Integral 2: \(\int_{0}^{1} \arcsin^2(x) \, dx\)

To evaluate \(\int_{0}^{1} \arcsin^2(x) \, dx\), we use the substitution \(x = \sin(\theta)\), so \(dx = \cos(\theta) d\theta\) and \(\arcsin(x) = \theta\). The limits change from \(x = 0\) to \(\theta = 0\) and \(x = 1\) to \(\theta = \frac{\pi}{2}\):

\[
\int_{0}^{1} \arcsin^2(x) \, dx = \int_{0}^{\frac{\pi}{2}} \theta^2 \cos(\theta) \, d\theta
\]

We use integration by parts twice. Let \(u = \theta^2\) and \(dv = \cos(\theta) d\theta\). Then \(du = 2\theta d\theta\) and \(v = \sin(\theta)\):

\[
\int \theta^2 \cos(\theta) \, d\theta = \theta^2 \sin(\theta) - \int 2\theta \sin(\theta) \, d\theta
\]

For the remaining integral, let \(u = \theta\) and \(dv = \sin(\theta) d\theta\). Then \(du = d\theta\) and \(v = -\cos(\theta)\):

\[
\int \theta \sin(\theta) \, d\theta = -\theta \cos(\theta) + \int \cos(\theta) \, d\theta = -\theta \cos(\theta) + \sin(\theta)
\]

Thus,

\[
\int \theta^2 \cos(\theta) \, d\theta = \theta^2 \sin(\theta) + 2\theta \cos(\theta) - 2\sin(\theta) + C
\]

Evaluating from 0 to \(\frac{\pi}{2}\):

\[
\int_{0}^{\frac{\pi}{2}} \theta^2 \cos(\theta) \, d\theta = \left[ \theta^2 \sin(\theta) + 2\theta \cos(\theta) - 2\sin(\theta) \right]_{0}^{\frac{\pi}{2}} = \left( \frac{\pi^2}{4} \cdot 1 + 2 \cdot \frac{\pi}{2} \cdot 0 - 2 \cdot 1 \right) - (0 + 0 - 0) = \frac{\pi^2}{4} - 2
\]

### Step 2: Combine the Results

Combining the results from the two integrals:

\[
\int_{0}^{1} \arcsin(x) \arccos(x) \, dx = \frac{\pi}{2} \left( \frac{\pi}{2} - 1 \right) - \left( \frac{\pi^2}{4} - 2 \right) = \frac{\pi^2}{4} - \frac{\pi}{2} - \frac{\pi^2}{4} + 2 = 2 - \frac{\pi}{2}
\]

### Step 3: Numerical Approximation

The numerical approximation of \(2 - \frac{\pi}{2}\) is:

\[
2 - \frac{\pi}{2} \approx 2 - 1.5707963267948966 = 0.4292036732051034
\]

### Step 4: Output the Final Answer

\[
\boxed{
\begin{aligned}
\text{"answer": "2 - \frac{\pi}{2}", "numerical_answer": "0.4292036732"}
\end{aligned}
}
\]