

To solve the definite integral \(\int\limits_0^{2} x^{-1/2} \left[1 + \sqrt{x(2 - x)}\right]^{-3/2} \, dx\), we proceed with the following steps:

### Step 1: Substitution to Simplify the Integrand
First, observe that \(x(2 - x) = 2x - x^2 = 1 - (x - 1)^2\) (by completing the square). This suggests a trigonometric substitution. Let \(x = 1 + \sin\theta\), so \(dx = \cos\theta \, d\theta\). The limits of integration change as follows:
- When \(x = 0\), \(\sin\theta = -1 \implies \theta = -\frac{\pi}{2}\).
- When \(x = 2\), \(\sin\theta = 1 \implies \theta = \frac{\pi}{2}\).

### Step 2: Rewrite the Integrand
Under this substitution:
- \(x(2 - x) = (1 + \sin\theta)(1 - \sin\theta) = \cos^2\theta\), so \(\sqrt{x(2 - x)} = \cos\theta\) (since \(\cos\theta \geq 0\) for \(\theta \in [-\frac{\pi}{2}, \frac{\pi}{2}]\)).
- \(x^{-1/2} = (1 + \sin\theta)^{-1/2}\).
- The term \(\left[1 + \sqrt{x(2 - x)}\right]^{-3/2} = (1 + \cos\theta)^{-3/2}\).

Thus, the integrand becomes:
\[
(1 + \sin\theta)^{-1/2} \cdot (1 + \cos\theta)^{-3/2} \cdot \cos\theta \, d\theta
\]

### Step 3: Simplify Using Trigonometric Identities
Using identities:
- \(1 + \cos\theta = 2\cos^2\left(\frac{\theta}{2}\right)\), so \((1 + \cos\theta)^{-3/2} = 2^{-3/2} \cos^{-3}\left(\frac{\theta}{2}\right)\).
- \(1 + \sin\theta = \left(\sin\left(\frac{\theta}{2}\right) + \cos\left(\frac{\theta}{2}\right)\right)^2\), so \((1 + \sin\theta)^{-1/2} = \frac{1}{\sin\left(\frac{\theta}{2}\right) + \cos\left(\frac{\theta}{2}\right)}\).
- \(\cos\theta = \left(\cos\left(\frac{\theta}{2}\right) - \sin\left(\frac{\theta}{2}\right)\right)\left(\cos\left(\frac{\theta}{2}\right) + \sin\left(\frac{\theta}{2}\right)\right)\).

Substituting these into the integrand, the \(\sin\left(\frac{\theta}{2}\right) + \cos\left(\frac{\theta}{2}\right)\) terms cancel, leaving:
\[
2^{-3/2} \cdot \frac{\cos\left(\frac{\theta}{2}\right) - \sin\left(\frac{\theta}{2}\right)}{\cos^3\left(\frac{\theta}{2}\right)} \cdot d\theta
\]

### Step 4: Further Substitution and Integration
Let \(u = \frac{\theta}{2}\), so \(d\theta = 2du\) and the limits become \(u \in [-\frac{\pi}{4}, \frac{\pi}{4}]\). The integral simplifies to:
\[
\frac{1}{\sqrt{2}} \int_{-\frac{\pi}{4}}^{\frac{\pi}{4}} \left[\sec^2 u - \sec^3 u \sin u\right] du
\]

### Step 5: Evaluate the Integral
Split the integral into two parts:
- \(\int \sec^2 u \, du = \tan u\).
- \(\int \sec^3 u \sin u \, du = \int \tan u \sec^2 u \, du = \frac{1}{2} \sec^2 u\) (using \(v = \sec u\), \(dv = \sec u \tan u \, du\)).

Evaluating from \(-\frac{\pi}{4}\) to \(\frac{\pi}{4}\):
- At \(u = \frac{\pi}{4}\): \(\tan\left(\frac{\pi}{4}\right) = 1\), \(\frac{1}{2} \sec^2\left(\frac{\pi}{4}\right) = 1\), so \(1 - 1 = 0\).
- At \(u = -\frac{\pi}{4}\): \(\tan\left(-\frac{\pi}{4}\right) = -1\), \(\frac{1}{2} \sec^2\left(-\frac{\pi}{4}\right) = 1\), so \(-1 - 1 = -2\).

The difference is \(0 - (-2) = 2\). Multiplying by \(\frac{1}{\sqrt{2}}\) gives \(\sqrt{2}\).

### Final Result
The exact value of the integral is \(\sqrt{2}\), and its numerical approximation (rounded to 10 decimal places) is \(1.4142135624\).

{"answer": "\(\sqrt{2}\)", "numerical_answer": "1.4142135624"}