Let's compute the definite integral:
\[
I = \int_0^{1/2} \ln\left(\sqrt{1-x}-\sqrt{x}\right)\,dx
\]

## Step 1: Simplification via Substitution

Let’s attempt the substitution \( x = \sin^2 \theta \), with \( \theta \in [0, \pi/4] \):

- When \( x = 0 \), \( \theta = 0 \).
- When \( x = \frac{1}{2} \), \( \theta = \arcsin \left(\frac{1}{\sqrt{2}}\right) = \frac{\pi}{4} \).

Then,
\[
\sqrt{x} = \sin \theta, \quad \sqrt{1-x} = \cos \theta, \quad dx = 2\sin\theta \cos\theta\, d\theta = \sin 2\theta\, d\theta
\]

So the integrand becomes
\[
\ln(\sqrt{1-x} - \sqrt{x}) = \ln(\cos\theta - \sin\theta)
\]

Therefore,
\[
I = \int_{0}^{\pi/4} \ln(\cos\theta - \sin\theta) \cdot \sin 2\theta \, d\theta
\]

But \(\sin 2\theta = 2\sin\theta\cos\theta\), so we can write:
\[
I = \int_0^{\pi/4} 2\sin\theta\cos\theta \ln(\cos\theta - \sin\theta) d\theta
\]

## Step 2: Further simplification

Note that \(\cos\theta-\sin\theta = \sqrt{2}\cos\left(\theta + \frac{\pi}{4}\right)\).

So,
\[
\ln(\cos\theta-\sin\theta) = \frac{1}{2}\ln 2 + \ln\left(\cos\left(\theta+\frac{\pi}{4}\right)\right)
\]
Thus,
\[
I = \int_0^{\pi/4} 2\sin\theta\cos\theta \left( \frac{1}{2}\ln 2 + \ln\cos\left(\theta+\frac{\pi}{4}\right) \right) d\theta
\]
\[
= \ln 2 \int_0^{\pi/4} \sin\theta \cos\theta\, d\theta + 2\int_0^{\pi/4} \sin\theta\cos\theta \ln\cos\left(\theta+\frac{\pi}{4}\right) d\theta
\]

But \(\sin\theta\cos\theta = \frac{1}{2}\sin 2\theta\), so:

First term:
\[
\int_0^{\pi/4}\sin\theta\cos\theta d\theta = \frac{1}{2}\int_0^{\pi/4} \sin 2\theta d\theta = \frac{1}{2}\left. \left(-\frac{1}{2}\cos 2\theta\right) \right|_0^{\pi/4} = -\frac{1}{4} [\cos(\pi/2) - \cos(0)] = -\frac{1}{4}(0 - 1) = \frac{1}{4}
\]

Thus, the first term is \(\ln 2 \cdot \frac{1}{4} = \frac{1}{4}\ln 2\).

Second term:
\[
2\int_0^{\pi/4} \sin\theta\cos\theta \ln\cos\left(\theta+\frac{\pi}{4}\right)\, d\theta 
= \int_0^{\pi/4} \sin 2\theta \ln\cos\left(\theta + \frac{\pi}{4}\right)\, d\theta
\]

Let’s perform the substitution \( \phi = \theta + \frac{\pi}{4} \Rightarrow d\phi = d\theta \).

\[
\theta = 0 \implies \phi = \frac{\pi}{4} \\
\theta = \frac{\pi}{4} \implies \phi = \frac{\pi}{2} \\
\]

Rewrite \( \sin 2\theta \) in terms of \( \phi \):
\[
2\theta = 2(\phi - \frac{\pi}{4}) = 2\phi - \frac{\pi}{2} \implies \sin 2\theta = \sin(2\phi - \frac{\pi}{2}) = -\cos 2\phi
\]

So, the integral becomes:
\[
\int_{0}^{\pi/4} \sin 2\theta \ln\cos\left(\theta+\frac{\pi}{4}\right) d\theta = \int_{\pi/4}^{\pi/2} -\cos 2\phi \ln\cos\phi d\phi
\]
\[
= -\int_{\pi/4}^{\pi/2} \cos 2\phi \ln\cos\phi d\phi
\]

Now, use the double-angle formula:
\[
\cos 2\phi = 2\cos^2\phi - 1
\]
So,
\[
-\int_{\pi/4}^{\pi/2} \cos 2\phi \ln\cos\phi d\phi = -2\int_{\pi/4}^{\pi/2} \cos^2\phi \ln\cos\phi d\phi + \int_{\pi/4}^{\pi/2} \ln\cos\phi d\phi
\]

Therefore,
\[
I = \frac{1}{4}\ln 2 -2\int_{\pi/4}^{\pi/2} \cos^2\phi \ln\cos\phi d\phi + \int_{\pi/4}^{\pi/2} \ln\cos\phi d\phi
\]

## Step 3: Evaluate \( \int_{\pi/4}^{\pi/2} \cos^2\phi \ln\cos\phi d\phi \)

Recall
\(
\cos^2\phi = \frac{1 + \cos 2\phi}{2}
\)
So
\[
\int \cos^2\phi \ln\cos\phi d\phi = \frac{1}{2} \int \ln\cos\phi d\phi + \frac{1}{2} \int \cos 2\phi \ln\cos\phi d\phi
\]

Let’s use this in our expression:

Let’s denote:
\[
J = \int_{\pi/4}^{\pi/2} \cos^2\phi \ln\cos\phi d\phi = \frac{1}{2}\int_{\pi/4}^{\pi/2} \ln\cos\phi d\phi + \frac{1}{2} K
\]
where
\[
K := \int_{\pi/4}^{\pi/2} \cos 2\phi \ln\cos\phi d\phi
\]

But look, our main integral is in terms of \( I \), with \( -2J \):

So,
\[
I = \frac{1}{4}\ln 2 -2J + \int_{\pi/4}^{\pi/2} \ln\cos\phi d\phi
\]
\[
= \frac{1}{4}\ln 2 -2\left[\frac{1}{2} \int_{\pi/4}^{\pi/2} \ln\cos\phi d\phi + \frac{1}{2}K\right] + \int_{\pi/4}^{\pi/2} \ln\cos\phi d\phi
\]
\[
= \frac{1}{4}\ln 2 - \int_{\pi/4}^{\pi/2} \ln\cos\phi d\phi - K + \int_{\pi/4}^{\pi/2} \ln\cos\phi d\phi
\]
\[
= \frac{1}{4}\ln 2 - K
\]

Because the two log-cosine terms cancel.

## Step 4: Final Simplified Integral

So we finally get:
\[
I = \frac{1}{4}\ln 2 - \int_{\pi/4}^{\pi/2} \cos 2\phi \ln\cos\phi d\phi
\]

Let's compute \( K \):
\[
K = \int_{\pi/4}^{\pi/2} \cos 2\phi \ln\cos\phi d\phi
\]

Let’s use integration by parts:
Let \( u = \ln\cos\phi \implies du = -\tan\phi d\phi \)
Let \( dv = \cos 2\phi d\phi \implies v = \frac{1}{2}\sin 2\phi \)

So,
\[
K = \int \cos 2\phi \ln\cos\phi d\phi = \frac{1}{2} \sin 2\phi \ln\cos\phi - \frac{1}{2}\int \sin 2\phi \cdot (-\tan\phi) d\phi
\]
\[
= \frac{1}{2} \sin 2\phi \ln\cos\phi + \frac{1}{2} \int \sin 2\phi \tan\phi d\phi
\]

But \(\sin 2\phi = 2\sin\phi\cos\phi\), and \( \tan\phi = \frac{\sin\phi}{\cos\phi} \):

\[
\sin 2\phi \tan\phi = 2\sin\phi\cos\phi \cdot \frac{\sin\phi}{\cos\phi} = 2\sin^2\phi
\]

So,
\[
K = \frac{1}{2} \sin 2\phi \ln\cos\phi + \frac{1}{2} \int 2\sin^2\phi d\phi
= \frac{1}{2} \sin 2\phi \ln\cos\phi + \int \sin^2\phi d\phi
\]

Therefore:

\[
K = \frac{1}{2} \sin 2\phi \ln\cos\phi + \int \sin^2\phi d\phi
\]

Between \(\phi = \frac{\pi}{4}\) and \(\phi = \frac{\pi}{2}\).

But

\[
\int \sin^2\phi d\phi = \frac{1}{2} \int (1-\cos 2\phi) d\phi = \frac{1}{2}\left[ \phi - \frac{1}{2}\sin 2\phi \right] + C
\]

Therefore, total:

\[
K = \frac{1}{2}\sin 2\phi \ln\cos\phi + \frac{1}{2}\phi - \frac{1}{4}\sin 2\phi
\Big|_{\pi/4}^{\pi/2}
\]

Let's compute the boundary values.

At \(\phi = \frac{\pi}{2}\):

- \(\sin 2\phi = \sin \pi = 0\)
- \(\ln\cos\phi = \ln(0) = -\infty\).
- But their product is \(0\) since \(\sin 2\phi = 0\).
- \(\phi = \frac{\pi}{2}\)
- \(\sin 2\phi = 0\)

At \(\phi = \frac{\pi}{4}\):

- \(\sin 2\phi = \sin \frac{\pi}{2} = 1\)
- \(\cos\phi = \cos\frac{\pi}{4} = \frac{1}{\sqrt{2}}\), so
- \(\ln\cos\phi = \ln\frac{1}{\sqrt{2}} = -\frac{1}{2}\ln 2\)
- \(\phi = \frac{\pi}{4}\)
- \(\sin 2\phi = 1\)

So, the evaluation at the limits:

\[
K = \left\{ \frac{1}{2} \cdot 0 \cdot \ln 0 + \frac{1}{2} \cdot \frac{\pi}{2} - \frac{1}{4}\cdot 0 \right\}
- \left\{ \frac{1}{2} \cdot 1 \cdot ( -\frac{1}{2} \ln 2 ) + \frac{1}{2} \cdot \frac{\pi}{4} - \frac{1}{4}\cdot 1 \right\}
\]

First term (upper limit) is:
\[
0 + \frac{\pi}{4} - 0 = \frac{\pi}{4}
\]

Second term (lower limit):
\[
\frac{1}{2} ( -\frac{1}{2}\ln 2 ) + \frac{1}{2}\cdot \frac{\pi}{4} - \frac{1}{4}
= -\frac{1}{4}\ln 2 + \frac{\pi}{8} - \frac{1}{4}
\]

Spelling out the minus sign:

\[
K = \frac{\pi}{4} - [ -\frac{1}{4}\ln 2 + \frac{\pi}{8} - \frac{1}{4} ]
= \frac{\pi}{4} + \frac{1}{4}\ln 2 - \frac{\pi}{8} + \frac{1}{4}
= \frac{\pi}{4} - \frac{\pi}{8} + \frac{1}{4} + \frac{1}{4}\ln 2
= \frac{\pi}{8} + \frac{1}{4} + \frac{1}{4}\ln 2
\]

## Step 5: Assemble the final result

Recall:
\[
I = \frac{1}{4}\ln 2 - K = \frac{1}{4}\ln 2 - \left( \frac{\pi}{8} + \frac{1}{4} + \frac{1}{4}\ln 2 \right)
= -\frac{\pi}{8} - \frac{1}{4}
\]

Therefore, the exact value is:
\[
\boxed{I = -\frac{\pi}{8} - \frac{1}{4}}
\]

## Step 6: Numerical approximation

Let’s compute this value numerically:

\[
\frac{\pi}{8} = \frac{3.141592653589793}{8} = 0.3926990817
\]
So,
\[
I = -0.3926990817 - 0.25 = -0.6426990817
\]

Rounded to 10 decimal places:
\[
I \approx -0.6426990817
\]

## Step 7: Final answer in JSON

```json
{"answer": "-\\frac{\\pi}{8} - \\frac{1}{4}", "numerical_answer": "-0.6426990817"}
```