<think>
Okay, let's see. I need to compute the definite integral from 0 to 1 of (1/x - floor(1/x)) dx. Hmm, floor function integrals can be tricky because they involve piecewise constant functions. Let me start by understanding the integrand.

The function inside the integral is 1/x minus the floor of 1/x. The floor function, floor(1/x), gives the greatest integer less than or equal to 1/x. So, for x in (0,1], 1/x ranges from 1 to infinity. Therefore, floor(1/x) will take integer values n where 1/(n+1) < x ≤ 1/n for each positive integer n.

Wait, so if I break the integral into intervals where floor(1/x) is constant, that might help. Let's consider substitution. Let me set t = 1/x, so x = 1/t and dx = -1/t² dt. When x approaches 0 from the right, t approaches infinity, and when x is 1, t is 1. So the integral becomes from t=1 to t=∞, but with the substitution, the negative sign will flip the limits. Let me check:

Original integral: ∫₀¹ (1/x - floor(1/x)) dx

Substitute x = 1/t, so dx = -1/t² dt. When x approaches 0, t approaches ∞; when x=1, t=1. So the integral becomes:

∫_{t=1}^{t=∞} (t - floor(t)) * (-1/t²) dt

But flipping the limits to make it from t=1 to t=∞, the negative goes away:

∫₁^∞ (t - floor(t)) * (1/t²) dt

So the integral is now from 1 to infinity of (t - floor(t))/t² dt. The term (t - floor(t)) is the fractional part of t, often written as {t}. So the integral becomes ∫₁^∞ {t}/t² dt.

Now, the fractional part {t} is t - n when t is in [n, n+1) for each integer n ≥ 1. So we can split the integral into a sum over intervals [n, n+1) for n from 1 to infinity. Therefore:

∫₁^∞ {t}/t² dt = Σₙ=₁^∞ ∫ₙ^{n+1} (t - n)/t² dt

Let me compute each integral in the sum. For each n, the integral from n to n+1 of (t - n)/t² dt. Let's make a substitution u = t - n, so when t = n, u=0; t = n+1, u=1. Then t = u + n, dt = du. The integral becomes:

∫₀¹ u/(u + n)² du

Hmm, integrating u/(u + n)² du. Let me try expanding this. Let me set v = u + n, so dv = du, and u = v - n. Then the integral becomes:

∫_{v=n}^{v=n+1} (v - n)/v² dv = ∫ₙ^{n+1} (v - n)/v² dv

Wait, that's the same as the original integral. Maybe another approach. Let's split the numerator:

u/(u + n)² = [ (u + n) - n ] / (u + n)² = 1/(u + n) - n/(u + n)²

So the integral becomes:

∫₀¹ [1/(u + n) - n/(u + n)²] du

Integrate term by term:

First term: ∫ 1/(u + n) du from 0 to1 is ln(u + n) from 0 to1 = ln(n +1) - ln(n)

Second term: ∫ n/(u + n)² du from 0 to1. The integral of n/(u + n)² is -n/(u + n) evaluated from 0 to1:

- n/(1 + n) + n/n = -n/(n +1) +1 = 1 - n/(n +1) = 1/(n +1)

So combining both terms:

[ln(n +1) - ln(n)] - [1/(n +1)]

Therefore, each integral in the sum is ln(n +1) - ln(n) - 1/(n +1)

So the total integral is Σₙ=₁^∞ [ln(n +1) - ln(n) - 1/(n +1)]

Let's write this sum as:

Σₙ=₁^∞ [ln((n +1)/n) - 1/(n +1)]

This can be split into two sums:

Σₙ=₁^∞ ln((n +1)/n) - Σₙ=₁^∞ 1/(n +1)

The first sum is a telescoping series. Let's expand the first few terms:

ln(2/1) + ln(3/2) + ln(4/3) + ... 

Each term cancels with the previous denominator, so the sum telescopes to lim_{N→∞} ln(N+1) - ln(1) = lim_{N→∞} ln(N+1) which diverges. Wait, but that can't be right because the original integral is convergent. Wait, but maybe I made a mistake here. Wait, the original integral was from 1 to infinity of {t}/t² dt. Since {t} is between 0 and 1, the integrand is O(1/t²), which is integrable at infinity. So the integral converges. Therefore, the sum must converge. But according to the first sum, Σ ln((n+1)/n) is divergent (harmonic series?), but the second sum Σ 1/(n+1) is also divergent. But their difference converges. Hmm, so we have two divergent series, but their difference converges. Let me check:

The first sum Σₙ=₁^∞ ln((n+1)/n) = Σₙ=₁^∞ [ln(n+1) - ln n] = lim_{N→∞} ln(N+1) - ln 1 = infinity. So it diverges to infinity.

The second sum Σₙ=₁^∞ 1/(n+1) = Σₖ=₂^∞ 1/k, which is the harmonic series minus the first term, so it diverges to infinity.

But their difference is infinity - infinity, which is indeterminate. Therefore, I must have made a mistake in splitting the sum. Wait, but the original integral is finite, so the sum must converge. Therefore, the approach of splitting into two sums is problematic here. Let me re-examine the expression.

Wait, the original sum is Σₙ=₁^∞ [ln(n +1) - ln(n) - 1/(n +1)]. Let's write this as:

lim_{N→∞} Σₙ=1^N [ln(n +1) - ln(n) - 1/(n +1)]

The sum Σₙ=1^N [ln(n +1) - ln(n)] telescopes to ln(N+1) - ln(1) = ln(N+1)

The sum Σₙ=1^N 1/(n +1) = Σₖ=2^{N+1} 1/k = H_{N+1} -1, where H_n is the nth harmonic number.

Therefore, the total sum is ln(N+1) - (H_{N+1} -1) = ln(N+1) - H_{N+1} +1

Now, as N approaches infinity, H_{N} ≈ ln N + γ + 1/(2N) - ..., where γ is the Euler-Mascheroni constant. So H_{N+1} ≈ ln(N+1) + γ + 1/(2(N+1)) - ...

Therefore, ln(N+1) - H_{N+1} ≈ ln(N+1) - [ln(N+1) + γ + 1/(2(N+1))] = -γ - 1/(2(N+1)) 

As N approaches infinity, the term becomes -γ. Therefore, the total sum becomes:

lim_{N→∞} [ln(N+1) - H_{N+1} +1] = (-γ) +1

Therefore, the integral is 1 - γ.

So the exact value of the integral is 1 minus the Euler-Mascheroni constant, which is approximately 1 - 0.5772156649... ≈ 0.4227843351.

Let me verify this result. The integral of the fractional part of t over t² from 1 to infinity equals 1 - γ. I recall that there is a known integral involving the fractional part function and the Euler-Mascheroni constant. Let me check if this is a standard result.

Yes, indeed, the integral ∫₁^∞ {t}/t² dt = 1 - γ. Therefore, the original integral from 0 to1 of (1/x - floor(1/x)) dx is equal to 1 - γ.

So the exact answer is 1 - γ, and numerically, γ ≈ 0.5772156649, so 1 - γ ≈ 0.4227843351. Rounded to 10 decimal places, that's 0.4227843351.

Therefore, the final answer is 1 - γ in LaTeX, which is 1 - \gamma, and the numerical approximation is approximately 0.4227843351.
</think>

{"answer": "1 - \\gamma", "numerical_answer": "0.4227843351"}