<think>
Okay, let's tackle this integral step by step. The problem is to compute the definite integral from 0 to 1.0 of x times the natural logarithm of (1.0 + sqrt(1.0^2 - x^2))/x, multiplied by the differential D(0.5x) dx. Hmm, first, I need to make sure I understand the notation here. The D(0.5x) part might be a bit confusing. Wait, in some contexts, D could represent the differential operator, but here it's probably a notation for the differential of 0.5x. So, D(0.5x) would be the derivative of 0.5x with respect to x, which is 0.5. So maybe the integral is actually ∫₀¹ x ln[(1 + √(1 - x²))/x] * 0.5 dx. Let me confirm that. If D(0.5x) is the differential, then d(0.5x) = 0.5 dx. So the integral becomes 0.5 ∫₀¹ x ln[(1 + √(1 - x²))/x] dx. That seems right.

So the integral simplifies to (0.5) times the integral from 0 to 1 of x ln[(1 + sqrt(1 - x²))/x] dx. Let me write that as (1/2) ∫₀¹ x ln[(1 + sqrt(1 - x²))/x] dx. Now, the challenge is to compute this integral analytically. Let's see. The integrand is x multiplied by a logarithm term. Maybe substitution would help here. Let's consider substitution to simplify the logarithm part.

First, let's look at the argument of the logarithm: (1 + sqrt(1 - x²))/x. Let me denote t = sqrt(1 - x²). Then, t = sqrt(1 - x²), so t² = 1 - x², which implies x² = 1 - t². Differentiating both sides, 2x dx = -2t dt, so x dx = -t dt. Hmm, but the integral has x dx, so maybe this substitution could be useful. Let's see. Let's try substituting t = sqrt(1 - x²). Then, when x = 0, t = 1, and when x = 1, t = 0. The limits would switch from 1 to 0. Let's see how the integrand transforms.

The logarithm term becomes ln[(1 + t)/x]. But x in terms of t is sqrt(1 - t²). Wait, no. Wait, t = sqrt(1 - x²), so x = sqrt(1 - t²). Therefore, the logarithm term is ln[(1 + t)/sqrt(1 - t²)]. Hmm, that might complicate things. Let's write that out. So substituting, the integral becomes:

Original integral (without the 1/2 factor) is ∫₀¹ x ln[(1 + t)/x] dx, which with substitution t = sqrt(1 - x²), x dx = -t dt, and limits from t=1 to t=0. So changing the limits, the integral becomes ∫₁⁰ [sqrt(1 - t²)] * ln[(1 + t)/sqrt(1 - t²)] * (-t dt). The negative sign flips the limits back to 0 to 1, so it's ∫₀¹ t sqrt(1 - t²) ln[(1 + t)/sqrt(1 - t²)] dt. Hmm, not sure if that's better. Maybe another substitution?

Alternatively, perhaps a trigonometric substitution. Let me try substituting x = sinθ. Then, when x = 0, θ = 0; x = 1, θ = π/2. Then sqrt(1 - x²) = cosθ. Let's see. Then dx = cosθ dθ. The integral becomes (1/2) ∫₀^{π/2} sinθ * ln[(1 + cosθ)/sinθ] * sinθ dθ. Wait, because x is sinθ, so x dx is sinθ * cosθ dθ. Wait, no. Wait, the original integrand is x ln(...) dx. So substituting x = sinθ, dx = cosθ dθ. So the integral (without the 1/2 factor) is ∫ sinθ * ln[(1 + cosθ)/sinθ] * cosθ dθ from 0 to π/2. So that's ∫₀^{π/2} sinθ cosθ ln[(1 + cosθ)/sinθ] dθ. Hmm, maybe that's manageable.

Let me simplify the logarithm term: ln[(1 + cosθ)/sinθ] = ln(1 + cosθ) - ln(sinθ). So the integral becomes ∫₀^{π/2} sinθ cosθ [ln(1 + cosθ) - ln(sinθ)] dθ. Let's split this into two integrals: I1 = ∫ sinθ cosθ ln(1 + cosθ) dθ and I2 = -∫ sinθ cosθ ln(sinθ) dθ. Let's compute I1 and I2 separately.

Starting with I1: Let u = 1 + cosθ. Then du/dθ = -sinθ. So sinθ dθ = -du. When θ = 0, u = 2; θ = π/2, u = 1. So I1 becomes ∫_{u=2}^{u=1} (u - 1) * (-du) * ln(u). Wait, because cosθ = u - 1. Wait, cosθ = u - 1? Wait, u = 1 + cosθ, so cosθ = u - 1. But in the integral, we have sinθ cosθ ln(1 + cosθ) dθ. Wait, sinθ cosθ dθ = cosθ * sinθ dθ. But with substitution u = 1 + cosθ, then du = -sinθ dθ. So sinθ dθ = -du. Then cosθ = u - 1. So the integral I1 becomes ∫_{2}^{1} (u - 1) * (-du) * ln u. The limits are from 2 to 1, so flipping them and removing the negative sign: ∫₁² (u - 1) ln u du. So I1 = ∫₁² (u - 1) ln u du.

Similarly, let's compute I2: -∫ sinθ cosθ ln(sinθ) dθ. Let me make substitution v = sinθ. Then dv = cosθ dθ. When θ = 0, v = 0; θ = π/2, v = 1. So the integral becomes -∫₀¹ v * ln v dv. Because sinθ = v, cosθ dθ = dv, so sinθ cosθ ln(sinθ) dθ = v * ln v * dv. So I2 = -∫₀¹ v ln v dv. That integral is a standard one. The integral of v ln v dv can be found by integration by parts. Let me recall that ∫ v ln v dv = (v²/2) ln v - ∫ (v²/2)(1/v) dv = (v²/2) ln v - (1/2) ∫ v dv = (v²/2) ln v - (1/4) v² + C. So evaluated from 0 to 1. At v=1: (1/2)(0) - (1/4)(1) = -1/4. At v=0: The limit as v approaches 0 of (v²/2 ln v - v²/4). The term v² ln v approaches 0 because ln v approaches -infinity, but v² approaches 0 faster. So the limit is 0 - 0 = 0. Therefore, ∫₀¹ v ln v dv = -1/4. Therefore, I2 = -(-1/4) = 1/4.

Now, back to I1: ∫₁² (u - 1) ln u du. Let's expand this integral. Let's split it into ∫₁² u ln u du - ∫₁² ln u du. Let's compute each part.

First integral: ∫ u ln u du. Integration by parts. Let w = ln u, dv = u du. Then dw = (1/u) du, v = u²/2. So ∫ u ln u du = (u²/2) ln u - ∫ (u²/2)(1/u) du = (u²/2) ln u - (1/2) ∫ u du = (u²/2) ln u - (1/4) u² + C.

Second integral: ∫ ln u du = u ln u - u + C.

So putting it all together, I1 = [ (u²/2 ln u - (1/4) u² ) from 1 to 2 ] - [ (u ln u - u ) from 1 to 2 ].

Compute the first part at u=2: (4/2 ln 2 - (1/4)*4) = 2 ln 2 - 1. At u=1: (1/2 ln 1 - 1/4) = 0 - 1/4. So the first part is (2 ln 2 - 1) - (-1/4) = 2 ln 2 - 1 + 1/4 = 2 ln 2 - 3/4.

Second part: At u=2: (2 ln 2 - 2). At u=1: (1*0 -1) = -1. So the second part is (2 ln 2 - 2) - (-1) = 2 ln 2 - 2 +1 = 2 ln 2 -1.

Therefore, I1 = (2 ln 2 - 3/4) - (2 ln 2 -1) = 2 ln 2 - 3/4 -2 ln 2 +1 = (2 ln 2 -2 ln 2) + (-3/4 +1) = 0 + 1/4 = 1/4.

Wait, that's interesting. So I1 = 1/4 and I2 = 1/4. Therefore, the original integral (without the 1/2 factor) is I1 + I2 = 1/4 + 1/4 = 1/2. Therefore, the entire integral with the 1/2 factor is (1/2)*(1/2) = 1/4. So the exact value is 1/4.

Wait, that seems surprisingly simple. Let me verify this again. Let's recap:

Original integral: (1/2) [I1 + I2] where I1 = 1/4 and I2 = 1/4. So (1/2)(1/4 +1/4) = (1/2)(1/2) = 1/4. So the exact answer is 1/4. Numerically, 1/4 is 0.25. So the numerical approximation would be 0.2500000000.

But let me check this with a numerical approximation to be sure. Let's compute the integral numerically. Let's take the original integral: (1/2) ∫₀¹ x ln[(1 + sqrt(1 - x²))/x] dx. Let's approximate this using a simple method, like midpoint rule with a few intervals, just to check.

Alternatively, since the exact answer is 1/4, which is 0.25, but let's see. Let's plug in x=0.5. The integrand at x=0.5: 0.5 * ln[(1 + sqrt(1 - 0.25))/0.5] = 0.5 * ln[(1 + sqrt(0.75))/0.5] = 0.5 * ln[(1 + (√3)/2)/0.5] = 0.5 * ln[(2 + √3)/1] ≈ 0.5 * ln(2 + 1.732) ≈ 0.5 * ln(3.732) ≈ 0.5 * 1.317 ≈ 0.6585. But the function's value at x=0.5 is about 0.6585. If we integrate from 0 to 1, but the exact answer is 0.25. Hmm, but integrating a function that's positive over the interval and getting 0.25 seems plausible. Let's do a rough numerical estimate. Let's approximate the integral using the trapezoidal rule with a few intervals.

Take n=2 intervals: points at 0, 0.5, 1. The function at x=0: x=0, the argument of ln is (1 + sqrt(1 -0))/0, which is (2)/0, which tends to infinity. But ln(inf) is infinity, but multiplied by x which is 0. So we have a 0*∞ indeterminate form. Let's compute the limit as x approaches 0+ of x ln[(1 + sqrt(1 -x²))/x]. Let me set x approaching 0. Let x approach 0, so sqrt(1 -x²) ≈1 - x²/2. Then (1 + sqrt(1 -x²))/x ≈ (2 - x²/2)/x ≈ 2/x - x/2. So ln(2/x - x/2) ≈ ln(2/x) + ln(1 - x²/(4)). As x approaches 0, the second term is negligible, so ln(2/x) ≈ ln(2) - ln x. Therefore, x ln(2/x) ≈ x ln2 - x ln x. As x approaches 0, x ln x approaches 0, so the limit is 0. Therefore, the integrand at x=0 is 0. So the function starts at 0, increases to some maximum, then decreases back to 0 at x=1? Wait, at x=1, the argument of the logarithm is (1 + 0)/1 =1, so ln(1)=0. So the integrand at x=1 is 1*0=0. So the function starts at 0, goes up, then back to 0. Let's compute at x=0.5, as before, the integrand is approximately 0.6585. Let's take another point, say x=0.7071 (sqrt(0.5)). Then sqrt(1 - x²) = sqrt(1 - 0.5) = sqrt(0.5) ≈0.7071. So the argument is (1 +0.7071)/0.7071 ≈1.7071/0.7071 ≈2.4142. ln(2.4142)≈0.88, so the integrand is 0.7071*0.88≈0.622. So the function is around 0.6-0.65 in the middle. If we use the trapezoidal rule with two intervals: h=0.5. The trapezoidal approximation would be h/2 [f(0) + 2f(0.5) + f(1)] = 0.5/2 [0 + 2*0.6585 +0] = 0.25 *1.317 ≈0.329. But the exact answer is 0.25. Hmm, this is higher. Maybe the function has a peak higher than 0.65. Let's check at x=0.3. x=0.3: sqrt(1 -0.09)=sqrt(0.91)=≈0.9539. So (1 +0.9539)/0.3≈1.9539/0.3≈6.513. ln(6.513)≈1.874. So integrand is 0.3*1.874≈0.562. At x=0.7: sqrt(1 -0.49)=sqrt(0.51)=≈0.7141. (1 +0.7141)/0.7≈1.7141/0.7≈2.4487. ln(2.4487)≈0.895. So integrand≈0.7*0.895≈0.6265. So maybe the function peaks around x=0.5 to x=0.7. Let's try Simpson's rule with more intervals. Let's take n=4 intervals, h=0.25. Points at 0, 0.25, 0.5, 0.75, 1. Compute f at each point:

x=0: 0.

x=0.25: 0.25 * ln[(1 + sqrt(1 -0.0625))/0.25] =0.25 * ln[(1 + sqrt(0.9375))/0.25] ≈0.25 * ln[(1 +0.9682)/0.25] ≈0.25 * ln(1.9682/0.25) ≈0.25 * ln(7.8728) ≈0.25 *2.063 ≈0.5158.

x=0.5: as before, ≈0.6585.

x=0.75: 0.75 * ln[(1 + sqrt(1 -0.5625))/0.75] =0.75 * ln[(1 + sqrt(0.4375))/0.75] ≈0.75 * ln[(1 +0.6614)/0.75] ≈0.75 * ln(1.6614/0.75) ≈0.75 * ln(2.2152) ≈0.75 *0.795 ≈0.596.

x=1:0.

Simpson's rule for n=4 (even number of intervals, so Simpson's 1/3 rule applies for the first two intervals and then Simpson's 3/8 for the last three? Wait, n=4, which is even, so Simpson's 1/3 can be applied. Wait, Simpson's rule requires even number of intervals. Wait, for n=4 intervals (5 points), Simpson's 1/3 rule can be applied as two applications of the rule. The formula is h/3 [f0 + 4f1 + 2f2 +4f3 + f4]. So h=0.25. So the integral approximation is 0.25/3 [0 +4*0.5158 +2*0.6585 +4*0.596 +0] ≈0.083333 [0 +2.0632 +1.317 +2.384 +0] ≈0.083333*(2.0632 +1.317=3.7642; 3.7642 +2.384=6.1482) ≈0.083333*6.1482≈0.51235. Then multiply by 1/2 (from the original integral's 1/2 factor) gives 0.256175. Hmm, which is close to 0.25. But the exact answer is 0.25. So with n=4, Simpson's rule gives approx 0.256, which is about 0.256, which is close to 0.25. Considering that Simpson's rule is exact for polynomials up to degree 3, but our integrand is not a polynomial, so the approximation is reasonable. Given that the exact answer is 1/4=0.25, and the numerical approximation with Simpson's rule is around 0.256, which is close. So this gives me more confidence that the exact answer is indeed 1/4.

Therefore, the exact answer is 1/4, and the numerical approximation is 0.2500000000.
</think>

{"answer": "\\frac{1}{4}", "numerical_answer": "0.2500000000"}