To solve the definite integral \(\int_{420}^{1672}\{\fracsqrt{\ln(2023-x)}}{\sqrt{\ln(2023-x)}+\sqrt{\ln(x-69)}}\:\mathrm{d}x\), we will follow the steps outlined.

### Step 1: Analytical Computation

Consider the integral:
\[ I = \int_{420}^{1672}\frac{\sqrt{\ln(2023-x)}}{\sqrt{\ln(2023-x)}+\sqrt{\ln(x-69)}}\:\mathrm{d}x. \]

To simplify this, we can use a symmetry argument. Let's make a substitution \( t = 2023 - x \). Then \( x = 2023 - t \) and \( dx = -dt \). The limits of integration change as follows:
- When \( x = 420 \), \( t = 2023 - 420 = 1603 \).
- When \( x = 1672 \), \( t = 2023 - 1672 = 351 \).

Thus, the integral becomes:
\[ I = \int_{1603}^{351}\frac{\sqrt{\ln t}}{\sqrt{\ln t}+\sqrt{\ln(2023 - (2023 - t))}}(-dt) = \int_{351}^{1603}\frac{\sqrt{\ln t}}{\sqrt{\ln t}+\sqrt{\ln(t-69)}}\:\mathrm{d}t. \]

Notice that the integrand is symmetric in \( x \) and \( t \). Therefore, we can write:
\[ I = \int_{420}^{1672}\frac{\sqrt{\ln(2023-x)}}{\sqrt{\ln(2023-x)}+\sqrt{\ln(x-69)}}\:\mathrm{d}x = \int_{420}^{1672}\frac{\sqrt{\ln(x-69)}}{\sqrt{\ln(x-69)}+\sqrt{\ln(2023-x)}}\:\mathrm{d}x. \]

Adding these two integrals, we get:
\[ 2I = \int_{420}^{1672}\left(\frac{\sqrt{\ln(2023-x)}}{\sqrt{\ln(2023-x)}+\sqrt{\ln(x-69)}} + \frac{\sqrt{\ln(x-69)}}{\sqrt{\ln(x-69)}+\sqrt{\ln(2023-x)}}\right)\:\mathrm{d}x. \]

Since the sum of the fractions is 1, we have:
\[ 2I = \int_{420}^{1672} 1 \:\mathrm{d}x = 1672 - 420 = 1252. \]

Thus,
\[ I = \frac{1252}{2} = 626. \]

### Step 2: Numerical Approximation

The numerical approximation of 626 is simply 626.0000000000.

### Step 3: JSON Output

The final answer in the required JSON format is:
```json
{"answer": "626", "numerical_answer": "626.0000000000"}
```