To solve the definite integral 

\[
\int_{1.0}^\infty x(x^2 - 1.0^2)^{2 - 3/2} e^{-0.5^2 x^2} H_{2*2}(0.5x) \, dx,
\]

let's break it down step by step.

### Step 1: Simplify the Integrand
First, simplify the terms in the integrand:

1. \((x^2 - 1.0^2)^{2 - 3/2} = (x^2 - 1)^{-1/2} = \frac{1}{\sqrt{x^2 - 1}}\).
2. \(H_{2*2}(0.5x) = H_4(0.5x)\), where \(H_4\) is the 4th-order Hermite polynomial.
3. The Hermite polynomial \(H_4(y)\) is given by:
   \[
   H_4(y) = 16y^4 - 48y^2 + 12.
   \]
   Substituting \(y = 0.5x\):
   \[
   H_4(0.5x) = 16(0.5x)^4 - 48(0.5x)^2 + 12 = x^4 - 6x^2 + 12.
   \]
4. The exponential term is \(e^{-0.25x^2}\).

Thus, the integrand simplifies to:
\[
x \cdot \frac{1}{\sqrt{x^2 - 1}} \cdot e^{-0.25x^2} \cdot (x^4 - 6x^2 + 12).
\]

### Step 2: Rewrite the Integral
The integral becomes:
\[
\int_{1.0}^\infty \frac{x(x^4 - 6x^2 + 12)}{\sqrt{x^2 - 1}} e^{-0.25x^2} \, dx.
\]

### Step 3: Change of Variables
Let \(u = x^2 - 1\), so \(du = 2x \, dx\) and \(x \, dx = \frac{du}{2}\). The limits change as follows:
- When \(x = 1\), \(u = 0\).
- When \(x \to \infty\), \(u \to \infty\).

The integral becomes:
\[
\int_{0}^\infty \frac{(u + 1)^2 - 6(u + 1) + 12}{2\sqrt{u}} e^{-0.25(u + 1)} \, du.
\]
Simplify the numerator:
\[
(u + 1)^2 - 6(u + 1) + 12 = u^2 + 2u + 1 - 6u - 6 + 12 = u^2 - 4u + 7.
\]
Thus, the integral is:
\[
\frac{1}{2} \int_{0}^\infty \frac{u^2 - 4u + 7}{\sqrt{u}} e^{-0.25(u + 1)} \, du.
\]

### Step 4: Split the Integral
Split the integral into three parts:
\[
\frac{1}{2} e^{-0.25} \left( \int_{0}^\infty u^{3/2} e^{-0.25u} \, du - 4 \int_{0}^\infty u^{1/2} e^{-0.25u} \, du + 7 \int_{0}^\infty u^{-1/2} e^{-0.25u} \, du \right).
\]

### Step 5: Evaluate the Integrals
Each integral is a gamma function \(\Gamma(n)\) where \(n\) is the exponent of \(u\) plus 1:
1. \(\int_{0}^\infty u^{3/2} e^{-0.25u} \, du = \Gamma(5/2) / (0.25)^{5/2}\),
2. \(\int_{0}^\infty u^{1/2} e^{-0.25u} \, du = \Gamma(3/2) / (0.25)^{3/2}\),
3. \(\int_{0}^\infty u^{-1/2} e^{-0.25u} \, du = \Gamma(1/2) / (0.25)^{1/2}\).

The gamma function values are:
- \(\Gamma(5/2) = \frac{3\sqrt{\pi}}{4}\),
- \(\Gamma(3/2) = \frac{\sqrt{\pi}}{2}\),
- \(\Gamma(1/2) = \sqrt{\pi}\).

Substituting these:
1. \(\Gamma(5/2) / (0.25)^{5/2} = \frac{3\sqrt{\pi}}{4} \cdot 32 = 24\sqrt{\pi}\),
2. \(\Gamma(3/2) / (0.25)^{3/2} = \frac{\sqrt{\pi}}{2} \cdot 8 = 4\sqrt{\pi}\),
3. \(\Gamma(1/2) / (0.25)^{1/2} = \sqrt{\pi} \cdot 2 = 2\sqrt{\pi}\).

Now, combine them:
\[
\frac{1}{2} e^{-0.25} \left( 24\sqrt{\pi} - 4 \cdot 4\sqrt{\pi} + 7 \cdot 2\sqrt{\pi} \right) = \frac{1}{2} e^{-0.25} \left( 24\sqrt{\pi} - 16\sqrt{\pi} + 14\sqrt{\pi} \right) = \frac{1}{2} e^{-0.25} \cdot 22\sqrt{\pi} = 11\sqrt{\pi} e^{-0.25}.
\]

### Step 6: Numerical Approximation
Compute the numerical value:
\[
11\sqrt{\pi} e^{-0.25} \approx 11 \cdot 1.77245385091 \cdot 0.77880078307 \approx 15.1969265046.
\]

### Final Answer
The exact answer is \(11\sqrt{\pi} e^{-1/4}\), and the numerical approximation is approximately \(15.1969265046\).

```json
{"answer": "11\\sqrt{\\pi} e^{-1/4}", "numerical_answer": "15.1969265046"}
```