
To solve the definite integral \(\int\limits_0^{2} x^{-1/2} \left[1 + \sqrt{x(2 - x)}\right]^{-3/2} \, dx\), we proceed with the following steps:

### Step 1: Trigonometric Substitution
First, observe that \(x(2 - x) = 1 - (x - 1)^2\) (by completing the square). This suggests a trigonometric substitution. Let \(x = 1 + \sin\theta\), so \(dx = \cos\theta \, d\theta\). The limits of integration transform as follows:
- When \(x = 0\), \(\sin\theta = -1 \implies \theta = -\pi/2\).
- When \(x = 2\), \(\sin\theta = 1 \implies \theta = \pi/2\).

### Step 2: Simplify the Integrand
Under this substitution:
- \(x(2 - x) = (1 + \sin\theta)(1 - \sin\theta) = 1 - \sin^2\theta = \cos^2\theta\), so \(\sqrt{x(2 - x)} = \cos\theta\) (since \(\cos\theta \geq 0\) for \(\theta \in [-\pi/2, \pi/2]\)).
- \(x = 1 + \sin\theta\), so \(x^{-1/2} = (1 + \sin\theta)^{-1/2}\).

The integrand becomes:
\[
(1 + \sin\theta)^{-1/2} \cdot (1 + \cos\theta)^{-3/2} \cdot \cos\theta \, d\theta
\]

### Step 3: Use Trigonometric Identities
Using the identities:
- \(1 + \sin\theta = (\sin(\theta/2) + \cos(\theta/2))^2\), so \((1 + \sin\theta)^{-1/2} = \frac{1}{\sin(\theta/2) + \cos(\theta/2)}\).
- \(1 + \cos\theta = 2\cos^2(\theta/2)\), so \((1 + \cos\theta)^{-3/2} = 2^{-3/2} \cos^{-3}(\theta/2)\).
- \(\cos\theta = (\cos(\theta/2) - \sin(\theta/2))(\cos(\theta/2) + \sin(\theta/2))\).

Substituting these into the integrand, the \((\sin(\theta/2) + \cos(\theta/2))\) terms cancel, leaving:
\[
2^{-3/2} \cdot \frac{\cos(\theta/2) - \sin(\theta/2)}{\cos^3(\theta/2)} \, d\theta
\]

### Step 4: Further Substitution
Let \(u = \theta/2\), so \(d\theta = 2 \, du\) and the limits become \(u \in [-\pi/4, \pi/4]\). The integral simplifies to:
\[
\frac{1}{\sqrt{2}} \int_{-\pi/4}^{\pi/4} \left( \sec^2 u - \tan u \sec^2 u \right) du
\]

### Step 5: Evaluate the Integral
The integral splits into two parts:
- \(\int \sec^2 u \, du = \tan u\)
- \(\int \tan u \sec^2 u \, du = \frac{1}{2} \tan^2 u\)

Evaluating from \(-\pi/4\) to \(\pi/4\):
\[
\frac{1}{\sqrt{2}} \left[ \left( \tan u - \frac{1}{2} \tan^2 u \right) \bigg|_{-\pi/4}^{\pi/4} \right] = \frac{1}{\sqrt{2}} \cdot 2 = \sqrt{2}
\]

### Numerical Approximation
The exact value is \(\sqrt{2}\), and its numerical approximation to 10 decimal places is \(1.4142135624\).

{"answer": "\(\sqrt{2}\)", "numerical_answer": "1.4142135624"}