To solve the definite integral \(\int\limits_{0}^{2}x\arctan\left(\sqrt{x(2-x)}\right)\,dx\), we will follow these steps:

### Step 1: Simplify the Integrand
First, observe that the expression inside the arctangent can be rewritten:
\[
\sqrt{x(2 - x)} = \sqrt{2x - x^2} = \sqrt{1 - (x - 1)^2}.
\]
This suggests a substitution to simplify the integral.

### Step 2: Substitution
Let \( u = x - 1 \). Then \( du = dx \), and when \( x = 0 \), \( u = -1 \); when \( x = 2 \), \( u = 1 \). The integral becomes:
\[
\int_{-1}^{1} (u + 1) \arctan\left(\sqrt{1 - u^2}\right) \, du.
\]
Notice that the integrand is an even function in \( u \) because \( \arctan\left(\sqrt{1 - u^2}\right) \) is even and \( u \) is odd. Thus, the integral simplifies to:
\[
2 \int_{0}^{1} \arctan\left(\sqrt{1 - u^2}\right) \, du.
\]

### Step 3: Further Simplification
Let \( u = \sin \theta \). Then \( du = \cos \theta \, d\theta \), and when \( u = 0 \), \( \theta = 0 \); when \( u = 1 \), \( \theta = \frac{\pi}{2} \). The integral becomes:
\[
2 \int_{0}^{\frac{\pi}{2}} \arctan\left(\sqrt{1 - \sin^2 \theta}\right) \cos \theta \, d\theta = 2 \int_{0}^{\frac{\pi}{2}} \arctan(\cos \theta) \cos \theta \, d\theta.
\]

### Step 4: Integration by Parts
Let \( v = \arctan(\cos \theta) \) and \( dw = \cos \theta \, d\theta \). Then \( dv = -\frac{\sin \theta}{1 + \cos^2 \theta} \, d\theta \) and \( w = \sin \theta \). Applying integration by parts:
\[
2 \left[ \sin \theta \arctan(\cos \theta) \Big|_{0}^{\frac{\pi}{2}} + \int_{0}^{\frac{\pi}{2}} \frac{\sin^2 \theta}{1 + \cos^2 \theta} \, d\theta \right].
\]
The boundary term evaluates to zero because \( \sin \frac{\pi}{2} = 1 \), \( \arctan(0) = 0 \), and \( \sin 0 = 0 \). Thus, we are left with:
\[
2 \int_{0}^{\frac{\pi}{2}} \frac{\sin^2 \theta}{1 + \cos^2 \theta} \, d\theta.
\]

### Step 5: Simplify the Remaining Integral
Using the identity \( \sin^2 \theta = 1 - \cos^2 \theta \), the integral becomes:
\[
2 \int_{0}^{\frac{\pi}{2}} \frac{1 - \cos^2 \theta}{1 + \cos^2 \theta} \, d\theta = 2 \int_{0}^{\frac{\pi}{2}} \left( \frac{2}{1 + \cos^2 \theta} - 1 \right) \, d\theta.
\]
Thus:
\[
4 \int_{0}^{\frac{\pi}{2}} \frac{1}{1 + \cos^2 \theta} \, d\theta - 2 \cdot \frac{\pi}{2} = 4 I - \pi,
\]
where \( I = \int_{0}^{\frac{\pi}{2}} \frac{1}{1 + \cos^2 \theta} \, d\theta \).

### Step 6: Evaluate \( I \)
To evaluate \( I \), use the substitution \( t = \tan \theta \). Then \( d\theta = \frac{dt}{1 + t^2} \), and \( \cos^2 \theta = \frac{1}{1 + t^2} \). The integral becomes:
\[
I = \int_{0}^{\infty} \frac{1}{1 + \frac{1}{1 + t^2}} \cdot \frac{dt}{1 + t^2} = \int_{0}^{\infty} \frac{dt}{2 + t^2} = \frac{1}{\sqrt{2}} \arctan\left(\frac{t}{\sqrt{2}}\right) \Big|_{0}^{\infty} = \frac{\pi}{2\sqrt{2}}.
\]

### Step 7: Combine Results
Substituting back:
\[
4 I - \pi = 4 \cdot \frac{\pi}{2\sqrt{2}} - \pi = \frac{2\pi}{\sqrt{2}} - \pi = \pi \left( \sqrt{2} - 1 \right).
\]

### Numerical Approximation
The numerical value of \( \pi \left( \sqrt{2} - 1 \right) \) is approximately:
\[
3.1415926536 \times (1.4142135624 - 1) \approx 1.3010767194.
\]

### Final Answer
```json
{"answer": "\\pi \\left( \\sqrt{2} - 1 \\right)", "numerical_answer": "1.3010767194"}
```