
To solve the definite integral \(\int\limits_0^{2} \sqrt{x(2-x)} \cos\left(\sqrt{x(2-x)}\right) \, dx\), we proceed with the following steps:


### Step 1: Simplify the Integrand and Substitute
First, observe that \(x(2-x) = 1 - (x-1)^2\) (by completing the square). This suggests a trigonometric substitution. Let \(x = 1 + \sin\theta\), so \(dx = \cos\theta \, d\theta\). When \(x = 0\), \(\theta = -\pi/2\); when \(x = 2\), \(\theta = \pi/2\). Substituting, we find:
\[
\sqrt{x(2-x)} = \sqrt{1 - \sin^2\theta} = \cos\theta
\]
Thus, the integrand becomes \(\cos\theta \cdot \cos(\cos\theta) \cdot \cos\theta \, d\theta = \cos^2\theta \cos(\cos\theta) \, d\theta\). The integral simplifies to:
\[
\int_{-\pi/2}^{\pi/2} \cos^2\theta \cos(\cos\theta) \, d\theta
\]
Since the integrand is even, this equals \(2 \int_0^{\pi/2} \cos^2\theta \cos(\cos\theta) \, d\theta\).


### Step 2: Use Bessel Function Integral Representations
Next, we use the identity \(\cos^2\theta = \frac{1 - \cos(2\theta)}{2}\) to rewrite the integral:
\[
\int_0^\pi \sin^2\phi \cos(\sin\phi) \, d\phi
\]
(by substituting \(\phi = 2\theta\)). Using the Fourier series expansion of \(\cos(\sin\phi)\) and properties of Bessel functions, we leverage the integral representation of Bessel functions:
\[
\int_0^\pi \cos(z \sin\phi) \, d\phi = \pi J_0(z)
\]
where \(J_0(z)\) is the Bessel function of the first kind of order 0. For \(z = 1\), this gives \(\int_0^\pi \cos(\sin\phi) \, d\phi = \pi J_0(1)\).


### Step 3: Evaluate the Integral Using Bessel Function Recurrence
The integral simplifies to:
\[
\frac{\pi}{2} \left( J_0(1) - J_2(1) \right)
\]
where \(J_2(1)\) is the Bessel function of the first kind of order 2 at \(z = 1\).


### Step 4: Numerical Approximation
Using known values of Bessel functions:
- \(J_0(1) \approx 0.7651976865579666\)
- \(J_2(1) \approx 0.11490348493190048\)

Thus:
\[
\frac{\pi}{2} \left( J_0(1) - J_2(1) \right) \approx \frac{\pi}{2} \left( 0.7651976865579666 - 0.11490348493190048 \right) \approx 1.0217344505
\]


### Final Answer
The exact answer is \(\frac{\pi}{2} \left( J_0(1) - J_2(1) \right)\), and the numerical approximation is approximately \(1.0217344505\).

{"answer": "\\frac{\\pi}{2} \\left( J_0(1) - J_2(1) \\right)", "numerical_answer": "1.0217344505"}