<think>
Okay, so I need to compute the definite integral from 0 to π/2 of [cos²x(1 + cosx)] divided by (1 + cosx + sinx) squared dx. Hmm, let's a bit intimidating at first glance. Let me break it down step by step.

First, the integrand is [cos²x(1 + cosx)] / (1 + cosx + sinx)². Maybe I can simplify the denominator first. Let me see if there's a substitution that can make this easier. The denominator is (1 + cosx + sinx)². Maybe if I let t = tan(x/2), which is the Weierstrass substitution. That often helps in integrals with sin and cos. Let me recall that substitution: sinx = 2t/(1 + t²), cosx = (1 - t²)/(1 + t²), and dx = 2/(1 + t²) dt. But before jumping into substitution, maybe there's another way.

Alternatively, perhaps expanding the denominator or numerator. Let me try to manipulate the denominator. Let's see, 1 + cosx + sinx. Maybe express this in terms of sin and cos. Alternatively, factor something out. Wait, 1 + cosx is 2cos²(x/2), and sinx is 2sin(x/2)cos(x/2). So maybe write the denominator as 2cos²(x/2) + 2sin(x/2)cos(x/2) = 2cos(x/2)(cos(x/2) + sin(x/2)). Then the denominator squared would be [2cos(x/2)(cos(x/2) + sin(x/2))]^2 = 4cos²(x/2)(cos(x/2) + sin(x/2))². Hmm, not sure if that helps yet.

Looking at the numerator: cos²x(1 + cosx). Let's see, cos²x is (1 + cos2x)/2, but maybe that's not helpful. Alternatively, 1 + cosx is 2cos²(x/2), so the numerator becomes cos²x * 2cos²(x/2). Wait, cosx is 2cos²(x/2) - 1, so cos²x would be (2cos²(x/2) - 1)^2. Hmm, that might complicate things. Maybe not the best approach.

Alternatively, let's consider substituting t = x - π/4. Sometimes shifting the variable can symmetrize the expression. But I'm not sure. Let me think. The denominator is 1 + cosx + sinx. If I write that as sqrt(2) sin(x + π/4) + 1? Wait, 1 + sinx + cosx. Let me compute sinx + cosx. That's sqrt(2) sin(x + π/4). So 1 + sqrt(2) sin(x + π/4). Hmm, maybe that's a way to write it, but I don't know if that helps.

Alternatively, let's try substitution u = 1 + cosx + sinx. Then du/dx = -sinx + cosx. Hmm, but the numerator is cos²x(1 + cosx). Not sure if that relates to du. Let me compute du: du = (cosx - sinx) dx. The integrand is [cos²x(1 + cosx)] / u². Maybe integrating by parts? Let me consider integrating by parts with u is the denominator part. Let me set v = 1/u, then dv = -1/u² du. But du is (cosx - sinx) dx. Hmm, not sure. Alternatively, maybe express the numerator in terms of u and du.

Wait, let's try to express the numerator in terms of u. Let's see, u = 1 + cosx + sinx. Let's compute u - 1 = cosx + sinx. Then (u - 1)^2 = cos²x + 2 sinx cosx + sin²x = 1 + sin2x. Hmm, not sure. Alternatively, maybe express cos²x in terms of u. Let's see, cos²x = (1 + cos2x)/2. But not sure.

Alternatively, let's consider multiplying numerator and denominator by (1 + cosx - sinx)^2 to rationalize. Wait, the denominator is (1 + cosx + sinx)^2. If I multiply numerator and denominator by (1 + cosx - sinx)^2, then denominator becomes [(1 + cosx)^2 - sin²x]^2. Let's compute that: (1 + cosx)^2 - sin²x = 1 + 2cosx + cos²x - sin²x. Since cos²x - sin²x = cos2x, so this becomes 1 + 2cosx + cos2x. Hmm, not sure if that's helpful. Let's compute it:

1 + 2cosx + cos2x. But cos2x = 2cos²x -1, so substituting: 1 + 2cosx + 2cos²x -1 = 2cosx + 2cos²x = 2cosx(1 + cosx). So the denominator after rationalization becomes [2cosx(1 + cosx)]². So the entire integrand becomes [cos²x(1 + cosx) * (1 + cosx - sinx)^2] / [2cosx(1 + cosx)]². Simplify numerator and denominator:

Numerator: cos²x(1 + cosx)(1 + cosx - sinx)^2

Denominator: 4cos²x(1 + cosx)^2

So cancelling terms: cos²x cancels, (1 + cosx) cancels once, so we have (1 + cosx - sinx)^2 / [4(1 + cosx)]

So the integrand simplifies to (1 + cosx - sinx)^2 / [4(1 + cosx)].

Hmm, that seems more manageable. Let me check that again. Original integrand: [cos²x(1 + cosx)] / (1 + cosx + sinx)^2. Multiply numerator and denominator by (1 + cosx - sinx)^2:

Numerator: cos²x(1 + cosx)(1 + cosx - sinx)^2

Denominator: [ (1 + cosx + sinx)(1 + cosx - sinx) ]^2 = [ (1 + cosx)^2 - sin²x ]^2 = [1 + 2cosx + cos²x - sin²x]^2. As before, that's [2cosx(1 + cosx)]^2. So denominator is 4cos²x(1 + cosx)^2. Then numerator over denominator is [cos²x(1 + cosx)(1 + cosx - sinx)^2] / [4cos²x(1 + cosx)^2] = (1 + cosx - sinx)^2 / [4(1 + cosx)].

So the integral becomes ∫ [ (1 + cosx - sinx)^2 / (4(1 + cosx)) ] dx from 0 to π/2. Let's factor out the 1/4: (1/4) ∫ (1 + cosx - sinx)^2 / (1 + cosx) dx.

Now, let's expand the numerator (1 + cosx - sinx)^2:

(1 + cosx - sinx)^2 = (1 + cosx)^2 - 2(1 + cosx)sinx + sin²x

Compute each term:

(1 + cosx)^2 = 1 + 2cosx + cos²x

-2(1 + cosx)sinx = -2sinx - 2sinx cosx

sin²x = sin²x

So adding all together:

1 + 2cosx + cos²x - 2sinx - 2sinx cosx + sin²x

Combine like terms:

1 + 2cosx + (cos²x + sin²x) - 2sinx - 2sinx cosx

Since cos²x + sin²x = 1, so:

1 + 2cosx + 1 - 2sinx - 2sinx cosx = 2 + 2cosx - 2sinx - 2sinx cosx

Factor out 2:

2[1 + cosx - sinx - sinx cosx]

So the integrand becomes (1/4) * [2(1 + cosx - sinx - sinx cosx)] / (1 + cosx) dx = (1/4)*2 [ (1 + cosx - sinx - sinx cosx) / (1 + cosx) ] dx = (1/2) ∫ [ (1 + cosx - sinx - sinx cosx) / (1 + cosx) ] dx

Now, split the fraction into terms:

= (1/2) ∫ [ (1 + cosx) - sinx(1 + cosx) ] / (1 + cosx) dx

Wait, let's see:

1 + cosx - sinx - sinx cosx = (1 + cosx) - sinx(1 + cosx)

Yes, factoring out (1 + cosx):

= (1 + cosx)(1 - sinx)

Therefore, the integrand becomes (1/2) ∫ [ (1 + cosx)(1 - sinx) / (1 + cosx) ] dx = (1/2) ∫ (1 - sinx) dx

Oh, that's a huge simplification! So after all that, the integral reduces to (1/2) times the integral of (1 - sinx) dx from 0 to π/2.

So now, ∫ (1 - sinx) dx = ∫1 dx - ∫ sinx dx = x + cosx + C

Therefore, the integral from 0 to π/2 is [x + cosx] evaluated from 0 to π/2.

Compute at π/2: π/2 + cos(π/2) = π/2 + 0 = π/2

Compute at 0: 0 + cos0 = 0 + 1 = 1

So the difference is π/2 - 1. Multiply by 1/2: (1/2)(π/2 - 1) = π/4 - 1/2

Wait, that seems too straightforward. Let me check if I made a mistake in the steps.

Wait, let's recap:

Original integral: ∫0^{π/2} [cos²x(1 + cosx)] / (1 + cosx + sinx)^2 dx

After substitution by multiplying numerator and denominator by (1 + cosx - sinx)^2, we simplified the integrand to (1/2) ∫ (1 - sinx) dx from 0 to π/2. Then integrating gives (1/2)(x + cosx) from 0 to π/2. Wait, but ∫(1 - sinx) dx is x + cosx, right? Because integral of 1 is x, integral of -sinx is cosx. So yes, [x + cosx] from 0 to π/2.

At upper limit: π/2 + cos(π/2) = π/2 + 0 = π/2

At lower limit: 0 + cos0 = 0 + 1 = 1

So difference is π/2 - 1. Multiply by 1/2: (π/2 - 1)/2 = π/4 - 1/2

So the exact answer is π/4 - 1/2. Let me check if that makes sense numerically. Let's compute π/4 ≈ 0.7854, 1/2 is 0.5, so 0.7854 - 0.5 ≈ 0.2854. Let me check with a quick numerical approximation.

Alternatively, maybe I made a mistake in the algebra when simplifying. Let me verify the step where I expanded (1 + cosx - sinx)^2.

Original expansion:

(1 + cosx - sinx)^2 = 1 + cos²x + sin²x + 2cosx - 2sinx - 2sinx cosx. Wait, wait, no. Wait, (a - b)^2 = a² - 2ab + b². So here, a = 1 + cosx, b = sinx. So (1 + cosx - sinx)^2 = (1 + cosx)^2 - 2(1 + cosx)sinx + sin²x. Then expanding (1 + cosx)^2 gives 1 + 2cosx + cos²x. Then subtract 2(1 + cosx)sinx: -2sinx - 2sinx cosx. Then add sin²x. So total is 1 + 2cosx + cos²x - 2sinx - 2sinx cosx + sin²x. Then cos²x + sin²x = 1, so that becomes 1 + 2cosx + 1 - 2sinx - 2sinx cosx = 2 + 2cosx - 2sinx - 2sinx cosx. Then factor out 2: 2[1 + cosx - sinx - sinx cosx]. Then when we divide by (1 + cosx), we have 2[1 + cosx - sinx - sinx cosx]/(1 + cosx). Then split into [ (1 + cosx) - sinx(1 + cosx) ] / (1 + cosx) = 1 - sinx. So yes, the integrand simplifies to 1 - sinx. Therefore, the integral becomes (1/2) ∫ (1 - sinx) dx. So the steps are correct.

Therefore, the exact value is π/4 - 1/2. Numerically, π is approximately 3.1415926536, so π/4 ≈ 0.7853981634, subtract 0.5 gives approximately 0.2853981634. Rounded to 10 decimal places, that's 0.2853981634.

Wait, but let me check with another approach. Let me compute the original integral numerically to verify. Let's take x from 0 to π/2, and compute the integrand [cos²x(1 + cosx)] / (1 + cosx + sinx)^2. Let's pick x = 0: cos0 = 1, sin0 = 0. So numerator is 1^2*(1 +1) = 2, denominator is (1 +1 +0)^2 = 4, so 2/4 = 0.5. At x = π/2: cos(π/2) = 0, so integrand is 0. So the integral starts at 0.5 and goes to 0. Let's see if the area under the curve is approximately 0.2854. Let's take a midpoint between 0 and π/2, say x = π/4. cos(π/4) = √2/2 ≈ 0.7071, sin(π/4) = √2/2. So numerator: (0.7071)^2*(1 + 0.7071) ≈ 0.5 * 1.7071 ≈ 0.8536. Denominator: (1 + 0.7071 + 0.7071)^2 = (1 + 1.4142)^2 ≈ (2.4142)^2 ≈ 5.8284. So integrand ≈ 0.8536 / 5.8284 ≈ 0.1464. So at x=π/4, the integrand is about 0.1464. So the integral from 0 to π/2 would be the average of the function times the interval? Not exactly, but since the function is decreasing from 0.5 to 0, maybe the integral is around 0.25 to 0.3. Which matches our previous result of ~0.2854. So that seems plausible.

Therefore, the exact answer is π/4 - 1/2, and the approximation is approximately 0.2853981634. So the final answer should be:

{"answer": "\frac{\pi}{4} - \frac{1}{2}", "numerical_answer": 0.2853981634}
</think>

{"answer": "\frac{\pi}{4} - \frac{1}{2}", "numerical_answer": 0.2853981634}