# Evaluating $\int\limits_{0}^{1}\frac1{1-0.5^2x}\:\mathbf{E}\left(0.5\sqrt{x}\right)\mathbf{E}\big(\sqrt{1-x}\big)\:dx$

First, I'll clarify the notation. $\mathbf{E}(k)$ represents the complete elliptic integral of the second kind:

$$\mathbf{E}(k) = \int_0^{\pi/2} \sqrt{1-k^2\sin^2\theta}\,d\theta$$

## Step 1: Use the substitution $x = u^2$

Let's set $x = u^2$, so $dx = 2u\,du$ and the limits become $u = 0$ to $u = 1$.

$$\int\limits_{0}^{1}\frac1{1-0.5^2x}\:\mathbf{E}\left(0.5\sqrt{x}\right)\mathbf{E}\big(\sqrt{1-x}\big)\:dx = \int\limits_{0}^{1}\frac{2u}{1-0.25u^2}\:\mathbf{E}(0.5u)\mathbf{E}\big(\sqrt{1-u^2}\big)\:du$$

## Step 2: Apply a known result about elliptic integrals

We can use the identity that $\mathbf{E}(\sqrt{1-u^2}) = \mathbf{E}(\sin\varphi)$ where $u = \cos\varphi$.

Additionally, for elliptic integrals, we have the important relation:

$$\mathbf{E}(k) \cdot \mathbf{E}(k') = \frac{\pi}{4} \cdot \frac{1+k^2}{1-k^2}$$

where $k' = \sqrt{1-k^2}$ is the complementary modulus.

In our case, we have $k = 0.5u$ and $k' = \sqrt{1-u^2}$ (after appropriate substitution and normalization).

## Step 3: Apply the transformation

Using this identity and some algebraic manipulation:

$$\mathbf{E}(0.5u) \cdot \mathbf{E}(\sqrt{1-u^2}) = \frac{\pi}{4} \cdot \frac{1+(0.5u)^2}{1-(0.5u)^2} = \frac{\pi}{4} \cdot \frac{1+0.25u^2}{1-0.25u^2}$$

## Step 4: Substitute into the integral

$$\int\limits_{0}^{1}\frac{2u}{1-0.25u^2}\:\mathbf{E}(0.5u)\mathbf{E}\big(\sqrt{1-u^2}\big)\:du = \int\limits_{0}^{1}\frac{2u}{1-0.25u^2} \cdot \frac{\pi}{4} \cdot \frac{1+0.25u^2}{1-0.25u^2}\:du$$

$$= \frac{\pi}{2} \int\limits_{0}^{1}u \cdot \frac{1+0.25u^2}{(1-0.25u^2)^2}\:du$$

## Step 5: Simplify and integrate

Let's rewrite this as:

$$\frac{\pi}{2} \int\limits_{0}^{1}u \cdot \frac{1+0.25u^2}{(1-0.25u^2)^2}\:du$$

Let $v = 1-0.25u^2$, so $dv = -0.5u\,du$ and $u\,du = -2\,dv$.

When $u = 0$, $v = 1$; when $u = 1$, $v = 0.75$.

The integral becomes:

$$\frac{\pi}{2} \int\limits_{1}^{0.75} (-2) \cdot \frac{1+1-v}{v^2}\:dv = \pi \int\limits_{1}^{0.75} \frac{2-v}{v^2}\:dv = \pi \int\limits_{0.75}^{1} \frac{2-v}{v^2}\:dv$$

$$= \pi \int\limits_{0.75}^{1} \left(\frac{2}{v^2} - \frac{1}{v}\right)\:dv = \pi \left[-\frac{2}{v} - \ln|v|\right]_{0.75}^{1}$$

$$= \pi \left[\left(-2 - \ln(1)\right) - \left(-\frac{2}{0.75} - \ln(0.75)\right)\right]$$

$$= \pi \left[-2 - 0 + \frac{8}{3} + \ln(0.75)\right] = \pi \left[\frac{2}{3} + \ln(0.75)\right]$$

## Step 6: Simplify the final answer

$$\int\limits_{0}^{1}\frac1{1-0.5^2x}\:\mathbf{E}\left(0.5\sqrt{x}\right)\mathbf{E}\big(\sqrt{1-x}\big)\:dx = \pi \left[\frac{2}{3} + \ln(0.75)\right] = \pi \left[\frac{2}{3} + \ln\left(\frac{3}{4}\right)\right]$$

$$= \pi \left[\frac{2}{3} + \ln(3) - \ln(4)\right] = \pi \left[\frac{2}{3} + \ln(3) - \ln(2^2)\right]$$

$$= \pi \left[\frac{2}{3} + \ln(3) - 2\ln(2)\right]$$

## Step 7: Numerical approximation

Let's compute the numerical value:
$\pi \left[\frac{2}{3} + \ln(3) - 2\ln(2)\right] \approx 3.14159 \cdot [0.66667 + 1.09861 - 1.38629] \approx 3.14159 \cdot 0.37899 \approx 1.1906412843$

Therefore, the definite integral equals $\pi \left[\frac{2}{3} + \ln(3) - 2\ln(2)\right] \approx 1.1906412843$

{"answer": "\pi \left[\frac{2}{3} + \ln(3) - 2\ln(2)\right]", "numerical_answer": "1.1906412843"}