To solve the definite integral 

\[
\int\limits_0^4 x^{-1/2}(4-x)^{-1/2}\left[1 - 0.25x(4-x)\right]^{1/2} \, dx,
\]

we proceed with the following steps:

### Step 1: Simplify the Integrand
First, observe that the integrand can be rewritten in a more symmetric form. Letâ€™s denote \( x = 4\sin^2\theta \), which implies \( dx = 8\sin\theta\cos\theta \, d\theta \). The limits of integration transform as follows:
- When \( x = 0 \), \( \theta = 0 \).
- When \( x = 4 \), \( \theta = \frac{\pi}{2} \).

Substituting \( x = 4\sin^2\theta \) into the integrand:

\[
x^{-1/2} = (4\sin^2\theta)^{-1/2} = \frac{1}{2\sin\theta},
\]
\[
(4 - x)^{-1/2} = (4 - 4\sin^2\theta)^{-1/2} = \frac{1}{2\cos\theta},
\]
\[
1 - 0.25x(4 - x) = 1 - \sin^2\theta \cos^2\theta.
\]

Thus, the integrand becomes:

\[
\frac{1}{2\sin\theta} \cdot \frac{1}{2\cos\theta} \cdot \sqrt{1 - \sin^2\theta \cos^2\theta} \cdot 8\sin\theta\cos\theta \, d\theta = 2 \sqrt{1 - \sin^2\theta \cos^2\theta} \, d\theta.
\]

### Step 2: Simplify the Expression Inside the Square Root
Notice that:

\[
1 - \sin^2\theta \cos^2\theta = \sin^2\theta + \cos^2\theta - \sin^2\theta \cos^2\theta = \sin^2\theta (1 - \cos^2\theta) + \cos^2\theta = \sin^2\theta \sin^2\theta + \cos^2\theta = \sin^4\theta + \cos^2\theta.
\]

However, a more useful identity is:

\[
1 - \sin^2\theta \cos^2\theta = \frac{3}{4} + \frac{1}{4}\cos(4\theta).
\]

This can be derived using double-angle identities:

\[
\sin^2\theta \cos^2\theta = \frac{1}{4}\sin^2(2\theta) = \frac{1}{8}(1 - \cos(4\theta)),
\]
\[
1 - \sin^2\theta \cos^2\theta = 1 - \frac{1}{8}(1 - \cos(4\theta)) = \frac{7}{8} + \frac{1}{8}\cos(4\theta).
\]

But this seems inconsistent. Alternatively, let's directly compute:

\[
\sqrt{1 - \sin^2\theta \cos^2\theta} = \sqrt{1 - \frac{1}{4}\sin^2(2\theta)}.
\]

### Step 3: Evaluate the Integral
The integral now becomes:

\[
\int_0^{\pi/2} 2 \sqrt{1 - \frac{1}{4}\sin^2(2\theta)} \, d\theta.
\]

Let \( \phi = 2\theta \), then \( d\phi = 2d\theta \), and the limits change to \( 0 \) and \( \pi \):

\[
\int_0^{\pi} \sqrt{1 - \frac{1}{4}\sin^2\phi} \, d\phi.
\]

This is an elliptic integral. Specifically, it can be expressed in terms of the complete elliptic integral of the second kind \( E(k) \):

\[
\int_0^{\pi} \sqrt{1 - k^2 \sin^2\phi} \, d\phi = 2E(k),
\]

where \( k = \frac{1}{2} \). Thus, the integral evaluates to:

\[
2E\left(\frac{1}{2}\right).
\]

The exact value of \( E\left(\frac{1}{2}\right) \) is:

\[
E\left(\frac{1}{2}\right) = \frac{\pi}{2} \,_2F_1\left(-\frac{1}{2}, \frac{1}{2}; 1; \frac{1}{4}\right),
\]

but more commonly, it is expressed as:

\[
E\left(\frac{1}{2}\right) = \frac{\sqrt{\pi} \Gamma\left(\frac{3}{4}\right)}{\Gamma\left(\frac{1}{4}\right)} + \frac{\Gamma\left(\frac{1}{4}\right)^2}{4\sqrt{2\pi}}.
\]

However, for practical purposes, we can use the numerical value of \( E\left(\frac{1}{2}\right) \approx 1.467462209 \).

Thus, the integral is:

\[
2 \times 1.467462209 \approx 2.934924418.
\]

### Step 4: Numerical Approximation
The numerical approximation of the integral, rounded to 10 decimal places, is:

\[
2.9349244180.
\]

### Final Answer
The exact answer is \( 2E\left(\frac{1}{2}\right) \), where \( E \) is the complete elliptic integral of the second kind. The numerical approximation is \( 2.9349244180 \).

```json
{"answer": "2E\\left(\\frac{1}{2}\\right)", "numerical_answer": "2.9349244180"}
```