
To solve the definite integral \(\int\limits_0^2 x^{-1/2} H_3\left(\sqrt[4]{x(2-x)}\right) dx\), we follow these steps:

### Step 1: Expand the Hermite Polynomial
The 3rd Hermite polynomial is \(H_3(z) = 8z^3 - 12z\). Substituting \(z = \sqrt[4]{x(2-x)}\), the integrand becomes:
\[
x^{-1/2} \left[8\left(x(2-x)\right)^{3/4} - 12\left(x(2-x)\right)^{1/4}\right]
\]

### Step 2: Simplify the Integral via Substitution
Let \(u = \sqrt{x}\), so \(x = u^2\) and \(dx = 2u \, du\). When \(x = 0\), \(u = 0\); when \(x = 2\), \(u = \sqrt{2}\). The integral transforms as:
\[
\int_0^2 x^{-1/2} H_3\left(\sqrt[4]{x(2-x)}\right) dx = 2 \int_0^{\sqrt{2}} H_3\left(\sqrt[4]{u^2(2 - u^2)}\right) du
\]

### Step 3: Evaluate the Transformed Integral
Substitute \(t = u^2/2\), so \(u = \sqrt{2t}\) and \(du = \frac{1}{\sqrt{2t}} dt\). The argument of the Hermite polynomial becomes \(\sqrt[4]{u^2(2 - u^2)} = \sqrt[4]{4t(1 - t)}\). The integral splits into two parts:
\[
2 \left[8 \int_0^{\sqrt{2}} \left(u^2(2 - u^2)\right)^{3/4} du - 12 \int_0^{\sqrt{2}} \left(u^2(2 - u^2)\right)^{1/4} du\right]
\]

### Step 4: Use Beta Function and Gamma Function
The integrals reduce to Beta functions \(B(a, b) = \int_0^1 t^{a-1}(1-t)^{b-1} dt = \frac{\Gamma(a)\Gamma(b)}{\Gamma(a+b)}\). After simplifying constants and using properties of the Gamma function (e.g., \(\Gamma(z)\Gamma(1-z) = \frac{\pi}{\sin(\pi z)}\)), the integrals evaluate to:
\[
8 \cdot \frac{3\pi\sqrt{2}}{16} - 12 \cdot \frac{\pi\sqrt{2}}{4} = -\frac{3\pi\sqrt{2}}{2}
\]

### Step 5: Final Result
Multiplying by the constant factor from the substitution, the exact integral is \(-3\pi\sqrt{2}\).

### Numerical Approximation
Using \(\pi \approx 3.141592653589793\) and \(\sqrt{2} \approx 1.4142135623730951\), the numerical value is approximately \(-13.3286487243\).

{"answer": "$-3\\pi\\sqrt{2}$", "numerical_answer": "-13.3286487243"}