<think>
Okay, so I need to compute the definite integral from 0 to 1 of arccos(x) times arctan(1.0x) dx. Hmm, let's start by understanding the problem. The integrand is the product of two inverse trigonometric functions: arccos(x) and arctan(x). Wait, the arctan has 1.0x, which is just x, right? So maybe the 1.0 is just there for clarity. Anyway, the integral is ∫₀¹ arccos(x) arctan(x) dx.

First, I remember that integrating products of functions often requires integration by parts. Let me recall the formula: ∫u dv = uv - ∫v du. So I need to choose which part to set as u and which as dv. Let's see, arccos(x) and arctan(x). Both are inverse trig functions, but their derivatives might be simpler. Let me check their derivatives.

The derivative of arccos(x) is -1/√(1 - x²), and the derivative of arctan(x) is 1/(1 + x²). Hmm, so if I let u be arccos(x), then du would be -1/√(1 - x²) dx. Then dv would be arctan(x) dx, so I need to find v by integrating arctan(x). Wait, but integrating arctan(x) is a standard integral. Let me recall: ∫arctan(x) dx. Let me do that first.

Let’s compute ∫arctan(x) dx. Let’s set w = arctan(x), dw = 1/(1 + x²) dx. Then, integration by parts: let’s set u1 = arctan(x), dv1 = dx. Then du1 = 1/(1 + x²) dx, v1 = x. So ∫arctan(x) dx = x arctan(x) - ∫x/(1 + x²) dx. The integral of x/(1 + x²) dx is (1/2) ln(1 + x²) + C. So overall, ∫arctan(x) dx = x arctan(x) - (1/2) ln(1 + x²) + C. Got that.

So if I take dv = arctan(x) dx, then v would be x arctan(x) - (1/2) ln(1 + x²). But maybe that's getting complicated. Alternatively, maybe I should set u = arccos(x) and dv = arctan(x) dx. Let me try that.

So, by parts: ∫arccos(x) arctan(x) dx from 0 to 1. Let u = arccos(x), dv = arctan(x) dx. Then du = -1/√(1 - x²) dx, and v = x arctan(x) - (1/2) ln(1 + x²). So applying integration by parts:

uv | from 0 to 1 - ∫v du. So that's [arccos(x) (x arctan(x) - (1/2) ln(1 + x²)) ) ] from 0 to 1 minus ∫ (x arctan(x) - (1/2) ln(1 + x²)) * (-1/√(1 - x²)) dx.

Wait, that seems a bit messy. Let me write that out step by step.

First, the boundary term:

At x = 1: arccos(1) is 0, so the first term is 0. At x = 0: arccos(0) is π/2. Then, the term is (π/2) * [0 * arctan(0) - (1/2) ln(1 + 0²)] = (π/2) * [0 - (1/2)*0] = 0. So the boundary term is 0 - 0 = 0. So the integral becomes - ∫ from 0 to1 of [x arctan(x) - (1/2) ln(1 + x²)] * (-1/√(1 - x²)) dx. The two negatives make it positive, so:

∫₀¹ [x arctan(x) - (1/2) ln(1 + x²)] / √(1 - x²) dx.

Hmm, so now the integral is split into two parts:

∫₀¹ [x arctan(x) / √(1 - x²)] dx - (1/2) ∫₀¹ [ln(1 + x²) / √(1 - x²)] dx.

Wait, no, actually, the first term is x arctan(x) over √(1 - x²), and the second term is (1/2) ln(1 + x²) over √(1 - x²). So the integral becomes:

∫₀¹ [x arctan(x) / √(1 - x²)] dx - (1/2) ∫₀¹ [ln(1 + x²) / √(1 - x²)] dx.

Hmm, this seems complicated. Let me denote the first integral as I1 and the second as I2. So the original integral is I1 - (1/2) I2.

Now, I need to compute I1 and I2. Let's start with I1: ∫₀¹ x arctan(x) / √(1 - x²) dx.

Hmm, maybe another integration by parts here? Let me see. Let’s set u = arctan(x), dv = x / √(1 - x²) dx. Then du = 1/(1 + x²) dx, and v = ?

Compute v: ∫ x / √(1 - x²) dx. Let’s set w = 1 - x², dw = -2x dx, so - (1/2) ∫ dw / √w = - (1/2) * 2√w + C = -√(1 - x²) + C. So v = -√(1 - x²).

So integration by parts for I1: u = arctan(x), dv = x / √(1 - x²) dx, then I1 = uv | from 0 to1 - ∫ v du.

So uv at 1: arctan(1) * (-√(1 - 1)) = (π/4)*0 = 0. At 0: arctan(0) * (-√(1 - 0)) = 0*(-1) = 0. So boundary term is 0. Then, - ∫ v du = - ∫ (-√(1 - x²)) * (1/(1 + x²)) dx = ∫ √(1 - x²)/(1 + x²) dx from 0 to1.

So I1 = ∫₀¹ √(1 - x²)/(1 + x²) dx.

Hmm, that's a different integral. Let me see how to compute that. Let’s make a substitution. Let’s set x = sinθ, so dx = cosθ dθ. Then √(1 - x²) = cosθ, and when x=0, θ=0; x=1, θ=π/2. So the integral becomes ∫₀^{π/2} cosθ / (1 + sin²θ) * cosθ dθ = ∫₀^{π/2} cos²θ / (1 + sin²θ) dθ.

Hmm, that's ∫ cos²θ / (1 + sin²θ) dθ. Let me see. Let's write cos²θ as 1 - sin²θ. So the integrand becomes (1 - sin²θ)/(1 + sin²θ) dθ. Let’s split the fraction: [1/(1 + sin²θ) - sin²θ/(1 + sin²θ)] dθ. Hmm, maybe that's helpful. Let me compute this integral.

Alternatively, use substitution. Let’s set t = tanθ, since we have trigonometric functions. Let’s try substitution t = tanθ. Then θ from 0 to π/2 corresponds to t from 0 to ∞. But maybe that's not helpful here. Alternatively, use substitution u = sinθ. Then du = cosθ dθ. But the denominator is 1 + u². Let me see:

∫ cos²θ / (1 + sin²θ) dθ = ∫ (1 - u²)/(1 + u²) * (du / cosθ). Wait, but cosθ = √(1 - u²). Hmm, this might complicate things. Alternatively, let's write the identity:

1 + sin²θ = 1 + (sin²θ - 1) +1? Not sure. Wait, perhaps use substitution t = tanθ. Let’s try:

Let t = tanθ, so θ from 0 to π/2 becomes t from 0 to ∞. Then sinθ = t / √(1 + t²), cosθ = 1 / √(1 + t²), dθ = dt / (1 + t²). So substituting into the integral:

∫₀^{∞} [ (1 / (1 + t²)) ] / [1 + (t² / (1 + t²)) ] * (dt / (1 + t²)) )

Wait, let's compute denominator 1 + sin²θ:

1 + sin²θ = 1 + t²/(1 + t²) = (1 + t² + t²)/(1 + t²) = (1 + 2t²)/(1 + t²). So the integrand becomes:

[cos²θ] / [1 + sin²θ] = [1/(1 + t²)] / [(1 + 2t²)/(1 + t²)] = 1/(1 + 2t²). Then multiplied by dθ = dt/(1 + t²). So the integral becomes ∫₀^∞ [1/(1 + 2t²)] * [1/(1 + t²)] dt. Hmm, so that's ∫₀^∞ 1 / [(1 + t²)(1 + 2t²)] dt.

This seems manageable. Let's use partial fractions. Let’s write 1 / [(1 + t²)(1 + 2t²)] = A/(1 + t²) + B/(1 + 2t²). Let's solve for A and B.

Multiply both sides by (1 + t²)(1 + 2t²):

1 = A(1 + 2t²) + B(1 + t²).

Set up equations by plugging in suitable t values. Let’s choose t² = -1/2, but that's complex. Alternatively, equate coefficients.

Expand the right side:

A(1) + A(2t²) + B(1) + B(t²) = (A + B) + (2A + B)t².

Set equal to left side, which is 1 = 0*t² + 1. So:

Coefficient of t²: 2A + B = 0.

Constant term: A + B = 1.

Solve the system:

From the first equation: B = -2A.

Substitute into the second: A - 2A = 1 => -A = 1 => A = -1. Then B = -2*(-1) = 2.

So the partial fractions decomposition is:

-1/(1 + t²) + 2/(1 + 2t²).

Therefore, the integral becomes:

∫₀^∞ [ -1/(1 + t²) + 2/(1 + 2t²) ] dt.

Integrate term by term:

- ∫₀^∞ 1/(1 + t²) dt + 2 ∫₀^∞ 1/(1 + 2t²) dt.

The first integral is - [ arctan(t) ] from 0 to ∞ = - (π/2 - 0) = -π/2.

The second integral: Let’s substitute u = t√2, so t = u/√2, dt = du/√2. Then:

2 ∫₀^∞ 1/(1 + 2t²) dt = 2 ∫₀^∞ 1/(1 + u²) * (du/√2) ) = 2/√2 ∫₀^∞ 1/(1 + u²) du = √2 [ arctan(u) ] from 0 to ∞ = √2 (π/2 - 0) = √2 π/2.

So the total is -π/2 + √2 π/2 = π/2 (√2 - 1).

Wait, √2 - 1? Let me check:

Wait, √2 π/2 - π/2 = π/2 (√2 - 1). Yes. So the integral I1 is equal to π/2 (√2 - 1).

Wait, but this was the integral for I1, which was ∫₀¹ √(1 - x²)/(1 + x²) dx. So I1 = π/2 (√2 - 1).

Okay, that's I1. Now, moving on to I2: ∫₀¹ [ln(1 + x²) / √(1 - x²)] dx.

Hmm, this integral looks tricky. Let me think. Let’s try substitution x = sinθ again. Then dx = cosθ dθ, √(1 - x²) = cosθ. So the integral becomes:

∫₀^{π/2} ln(1 + sin²θ) / cosθ * cosθ dθ = ∫₀^{π/2} ln(1 + sin²θ) dθ.

So I2 = ∫₀^{π/2} ln(1 + sin²θ) dθ. Hmm, how to compute this integral?

I recall that integrals involving ln(1 + a sin²θ) can sometimes be evaluated using series expansion or differentiation under the integral sign. Let me consider expanding ln(1 + sin²θ) into a power series.

We know that ln(1 + z) = Σ_{n=1}^∞ (-1)^{n+1} z^n / n for |z| < 1. Here, z = sin²θ, which is between 0 and 1 for real θ, so the series converges. So:

ln(1 + sin²θ) = Σ_{n=1}^∞ (-1)^{n+1} sin^{2n}θ / n.

Then, integrating term by term:

I2 = Σ_{n=1}^∞ [ (-1)^{n+1} / n ] ∫₀^{π/2} sin^{2n}θ dθ.

The integral ∫₀^{π/2} sin^{2n}θ dθ is known as the Wallis integral, which equals (π/2) * ( (2n)! ) / (4^n (n!)^2 ) ).

So substituting:

I2 = Σ_{n=1}^∞ [ (-1)^{n+1} / n ] * (π/2) * ( (2n)! ) / (4^n (n!)^2 ).

Hmm, this seems complicated, but maybe there's a closed-form expression for this series. Alternatively, perhaps we can relate it to known functions.

Alternatively, consider using differentiation under the integral sign. Let’s define a parameter a and consider the integral F(a) = ∫₀^{π/2} ln(1 + a sin²θ) dθ. Then, we can compute F'(a) = ∫₀^{π/2} [ sin²θ / (1 + a sin²θ) ] dθ. Then, I2 = F(1).

Let’s compute F'(a):

F'(a) = ∫₀^{π/2} sin²θ / (1 + a sin²θ) dθ.

Let’s make substitution t = tanθ, so θ from 0 to π/2 becomes t from 0 to ∞. Then sinθ = t / √(1 + t²), dθ = dt / (1 + t²).

So F'(a) = ∫₀^∞ [ (t² / (1 + t²)) / (1 + a (t² / (1 + t²)) ) ] * (dt / (1 + t²)).

Simplify the integrand:

Numerator: t² / (1 + t²)

Denominator: 1 + a t² / (1 + t²) = (1 + t² + a t²) / (1 + t²) = (1 + t²(1 + a)) / (1 + t²)

So the entire expression becomes:

[ t² / (1 + t²) ] / [ (1 + t²(1 + a)) / (1 + t²) ) ] * (1 / (1 + t²)) dt

Simplify:

= t² / (1 + t²(1 + a)) * 1/(1 + t²) dt

= t² / [ (1 + t²)(1 + (1 + a) t²) ] dt

= t² / [ (1 + t²)(1 + b t²) ] dt where b = 1 + a.

This seems like another partial fractions problem. Let’s decompose the integrand:

t² / [(1 + t²)(1 + b t²)] = A/(1 + t²) + B/(1 + b t²)

Multiply both sides by (1 + t²)(1 + b t²):

t² = A(1 + b t²) + B(1 + t²)

Expand:

t² = A + A b t² + B + B t²

Group terms:

t² (A b + B) + (A + B) = t²

So equate coefficients:

Coefficient of t²: A b + B = 1

Constant term: A + B = 0

From the second equation: B = -A. Substitute into the first equation:

A b - A = 1 => A (b - 1) = 1 => A = 1/(b - 1) = 1/(a + 1 - 1) = 1/a.

So A = 1/a, B = -1/a.

Therefore, the integrand becomes:

[1/(a (1 + t²))] - [1/(a (1 + b t²))] = (1/a)[1/(1 + t²) - 1/(1 + b t²)]

Therefore, F'(a) = (1/a) ∫₀^∞ [1/(1 + t²) - 1/(1 + b t²)] dt

Compute each integral:

∫₀^∞ 1/(1 + t²) dt = π/2

∫₀^∞ 1/(1 + b t²) dt = (1/√b) ∫₀^∞ 1/(1 + u²) du where u = t√b, so this is (1/√b)(π/2)

Thus, F'(a) = (1/a)[ π/2 - (1/√b)(π/2) ] = (π/(2a)) [1 - 1/√b]

But b = 1 + a, so:

F'(a) = (π/(2a)) [1 - 1/√(1 + a)]

Now, we need to integrate F'(a) to find F(a). Since I2 = F(1), we need to compute F(1) = ∫₀¹ F'(a) da + F(0). Wait, but when a=0, F(0) = ∫₀^{π/2} ln(1 + 0) dθ = 0. So F(1) = ∫₀¹ F'(a) da.

So F(1) = ∫₀¹ (π/(2a)) [1 - 1/√(1 + a)] da.

Let’s compute this integral:

F(1) = π/2 ∫₀¹ [1/a - 1/(a√(1 + a))] da.

Let’s split into two integrals:

π/2 [ ∫₀¹ 1/a da - ∫₀¹ 1/(a√(1 + a)) da ]

Wait, but ∫₀¹ 1/a da is problematic because it diverges. Wait, that can’t be right. There must be a mistake here. Because when a approaches 0, the original integral F(a) is ∫₀^{π/2} ln(1 + a sin²θ) dθ. As a approaches 0, this becomes ln(1) = 0, so F(0) = 0. But when we derived F'(a), we have an expression that seems to have a singularity at a=0. But since F(a) is well-behaved at a=0, the integral for F'(a) must also be finite. So perhaps there's a mistake in the partial fractions or the integration steps.

Wait, let's check the steps again. When we computed F'(a), we had:

F'(a) = (π/(2a)) [1 - 1/√(1 + a)]

But when a approaches 0, 1/√(1 + a) ≈ 1 - a/2 + 3a²/8 - ..., so 1 - 1/√(1 + a) ≈ a/2 - 3a²/8 + ... So F'(a) ≈ (π/(2a)) (a/2) ) = π/4 as a approaches 0, which is finite. So the integral ∫₀¹ F'(a) da is convergent.

So let's proceed. Let’s compute the two integrals:

First integral: ∫₀¹ 1/a da. This is divergent, but in our case, we have ∫₀¹ [1/a - 1/(a√(1 + a))] da. Let’s combine the terms:

1/a - 1/(a√(1 + a)) = [√(1 + a) - 1]/(a√(1 + a)).

Let’s make substitution t = √(1 + a). Let’s set t = √(1 + a), so t² = 1 + a, so a = t² - 1, da = 2t dt. When a=0, t=1; a=1, t=√2.

So the integral becomes:

∫_{t=1}^{√2} [ (t - 1) / ( (t² - 1) t ) ] * 2t dt = 2 ∫₁^{√2} (t - 1)/(t² - 1) dt.

Simplify (t² - 1) = (t - 1)(t + 1), so:

(t - 1)/(t² - 1) = 1/(t + 1).

So the integral becomes 2 ∫₁^{√2} 1/(t + 1) dt = 2 ln(t + 1) | from 1 to √2.

Evaluate:

2 [ ln(√2 + 1) - ln(2) ] = 2 ln( (√2 + 1)/2 ).

Therefore, the integral ∫₀¹ [1/a - 1/(a√(1 + a))] da = 2 ln( (√2 + 1)/2 ).

Thus, F(1) = π/2 * 2 ln( (√2 + 1)/2 ) = π ln( (√2 + 1)/2 ).

So I2 = π ln( (√2 + 1)/2 ).

Therefore, going back to the original integral:

Original integral = I1 - (1/2) I2 = π/2 (√2 - 1) - (1/2) π ln( (√2 + 1)/2 )

Simplify:

= (π/2)(√2 - 1) - (π/2) ln( (√2 + 1)/2 )

Factor out π/2:

= (π/2)[ (√2 - 1) - ln( (√2 + 1)/2 ) ]

So that's the exact analytical result.

Now, let's compute the numerical approximation. Let's compute each part:

First, compute √2 ≈ 1.41421356237

Then, √2 - 1 ≈ 0.41421356237

Next, compute (√2 + 1)/2 ≈ (1.41421356237 + 1)/2 ≈ 2.41421356237 / 2 ≈ 1.20710678119

Then, ln(1.20710678119) ≈ 0.18822610333

So, (√2 - 1) - ln(...) ≈ 0.41421356237 - 0.18822610333 ≈ 0.22598745904

Multiply by π/2 ≈ 1.57079632679 * 0.22598745904 ≈ 0.3549  (wait, let me compute more accurately)

Wait, 0.22598745904 * 1.57079632679:

First, 0.2 * 1.57079632679 = 0.314159265358

0.02598745904 * 1.57079632679 ≈ 0.02598745904 * 1.57079632679 ≈

Compute 0.02 * 1.57079632679 = 0.0314159265358

0.00598745904 * 1.57079632679 ≈ approx 0.00941 (since 0.005 * 1.5708 ≈ 0.009424)

So total ≈ 0.0314159265358 + 0.00941 ≈ 0.040825

So total ≈ 0.314159265358 + 0.040825 ≈ 0.354984

So the integral is approximately 0.354984. Let me check with a calculator for more precision.

Alternatively, use exact values:

Compute (√2 - 1) ≈ 0.4142135623730950488016887242097

ln( (√2 + 1)/2 ) ≈ ln(1.2071067811865475244008443621048) ≈ 0.18822610333443992431808955796418

So (√2 -1) - ln(...) ≈ 0.4142135623730950488016887242097 - 0.18822610333443992431808955796418 ≈ 0.2259874590386551244835991662455

Multiply by π/2 ≈ 1.5707963267948966192313216916398:

0.2259874590386551244835991662455 * 1.5707963267948966192313216916398 ≈

Let me compute this multiplication step by step:

0.2259874590386551244835991662455 * 1.5707963267948966192313216916398

First, 0.2 * 1.5707963267948966 = 0.3141592653589793

0.025987459038655124 * 1.5707963267948966 ≈

Compute 0.02 * 1.5707963267948966 = 0.03141592653589793

0.005987459038655124 * 1.5707963267948966 ≈

0.005 * 1.5707963267948966 = 0.007853981633974483

0.000987459038655124 * 1.5707963267948966 ≈ approx 0.001551

So total ≈ 0.007853981633974483 + 0.001551 ≈ 0.009404981633974483

So total for 0.025987459038655124 * 1.5707963267948966 ≈ 0.03141592653589793 + 0.009404981633974483 ≈ 0.04082090816987241

Adding to the 0.3141592653589793 gives 0.3141592653589793 + 0.04082090816987241 ≈ 0.3549801735288517

So approximately 0.3549801735. Rounded to 10 decimal places, that's 0.3549801735.

But let me verify this with a numerical integration method to check.

Alternatively, use a calculator for the exact expression:

The exact value is (π/2)[ (√2 -1) - ln( (√2 +1)/2 ) ]

Compute each part:

√2 ≈ 1.4142135623730950488016887242097

√2 -1 ≈ 0.4142135623730950488016887242097

(√2 +1)/2 ≈ (2.4142135623730950488016887242097)/2 ≈ 1.2071067811865475244008443621048

ln(1.2071067811865475244008443621048) ≈ 0.18822610333443992431808955796418

So (√2 -1) - ln(...) ≈ 0.4142135623730950488... - 0.1882261033344399243... ≈ 0.2259874590386551244835991662455

Multiply by π/2 ≈ 1.5707963267948966192313216916398:

0.2259874590386551244835991662455 * 1.5707963267948966192313216916398 ≈

Using a calculator:

0.2259874590386551244835991662455 * 1.5707963267948966192313216916398 ≈

Let me compute this using more precise steps:

First, write both numbers as:

0.2259874590386551244835991662455

and

1.5707963267948966192313216916398

Multiply:

0.2259874590386551244835991662455 × 1.5707963267948966192313216916398

Let me compute this step by step:

First, 0.2 × 1.5707963267948966 = 0.3141592653589793

0.025987459038655124 × 1.5707963267948966192313216916398

Break down 0.025987459038655124 into 0.02 + 0.005987459038655124

0.02 × 1.5707963267948966192313216916398 = 0.031415926535897932384626433832796

0.005987459038655124 × 1.5707963267948966192313216916398 ≈

Compute 0.005 × 1.5707963267948966192313216916398 = 0.00785398163397448309615608458199

0.000987459038655124 × 1.5707963267948966192313216916398 ≈

0.000987459038655124 × 1.5707963267948966192313216916398 ≈

Approximately 0.000987459038655124 × 1.5707963267948966 ≈ 0.001551

So total for 0.005987459038655124 × 1.5707963267948966 ≈ 0.007853981633974483 + 0.001551 ≈ 0.009404981633974483

Adding to the 0.031415926535897932 gives 0.031415926535897932 + 0.009404981633974483 ≈ 0.040820908169872415

Now, add this to the initial 0.3141592653589793:

0.3141592653589793 + 0.040820908169872415 ≈ 0.3549801735288517

So the exact value is approximately 0.3549801735288517. Rounded to 10 decimal places, that's 0.3549801735.

To confirm, let me use a numerical integration tool or calculator. Alternatively, compute using substitution.

Alternatively, use Wolfram Alpha to compute the original integral numerically. But since I can't access external tools, I'll proceed with the calculation.

Thus, the exact answer is (π/2)[ (√2 -1) - ln( (√2 +1)/2 ) ] and the numerical approximation is approximately 0.3549801735.

So the final answer in JSON should be:

{"answer": "\\frac{\\pi}{2} \\left( \\sqrt{2} - 1 - \\ln\\left( \\frac{\\sqrt{2} + 1}{2} \\right) \\right)", "numerical_answer": "0.3549801735"}

Let me check the LaTeX formatting:

The exact answer is written as \frac{\pi}{2} \left( \sqrt{2} - 1 - \ln\left( \frac{\sqrt{2} + 1}{2} \right) \right), which should be correct.
</think>

{"answer": "\\frac{\\pi}{2} \\left( \\sqrt{2} - 1 - \\ln\\left( \\frac{\\sqrt{2} + 1}{2} \\right) \\right)", "numerical_answer": "0.3549801735"}