To compute the definite integral 

\[
\int_0^1 \frac{e^{\arctan(x)}}{(x^2 + 1)^{3/2}} \, dx,
\]

we proceed with the following steps:

### Step 1: Substitution
Let \( u = \arctan(x) \). Then, the derivative of \( u \) with respect to \( x \) is:

\[
\frac{du}{dx} = \frac{1}{x^2 + 1} \implies du = \frac{dx}{x^2 + 1}.
\]

When \( x = 0 \), \( u = 0 \), and when \( x = 1 \), \( u = \frac{\pi}{4} \).

### Step 2: Rewrite the Integral
The integral becomes:

\[
\int_0^{\pi/4} \frac{e^u}{(x^2 + 1)^{1/2}} \, du.
\]

However, we need to express \( (x^2 + 1)^{1/2} \) in terms of \( u \). Since \( x = \tan(u) \), we have:

\[
x^2 + 1 = \tan^2(u) + 1 = \sec^2(u) \implies (x^2 + 1)^{1/2} = \sec(u).
\]

Thus, the integral simplifies to:

\[
\int_0^{\pi/4} \frac{e^u}{\sec(u)} \, du = \int_0^{\pi/4} e^u \cos(u) \, du.
\]

### Step 3: Integrate by Parts
To evaluate \( \int e^u \cos(u) \, du \), we use integration by parts twice. Let:

\[
I = \int e^u \cos(u) \, du.
\]

Let \( v = e^u \) and \( dw = \cos(u) \, du \). Then \( dv = e^u \, du \) and \( w = \sin(u) \). Applying integration by parts:

\[
I = e^u \sin(u) - \int e^u \sin(u) \, du.
\]

Now, apply integration by parts again to \( \int e^u \sin(u) \, du \). Let \( v = e^u \) and \( dw = \sin(u) \, du \). Then \( dv = e^u \, du \) and \( w = -\cos(u) \). Thus:

\[
\int e^u \sin(u) \, du = -e^u \cos(u) + \int e^u \cos(u) \, du = -e^u \cos(u) + I.
\]

Substituting back into the expression for \( I \):

\[
I = e^u \sin(u) - \left( -e^u \cos(u) + I \right) = e^u \sin(u) + e^u \cos(u) - I.
\]

Solving for \( I \):

\[
2I = e^u (\sin(u) + \cos(u)) \implies I = \frac{e^u (\sin(u) + \cos(u))}{2}.
\]

### Step 4: Evaluate the Definite Integral
Now, evaluate \( I \) from \( 0 \) to \( \pi/4 \):

\[
\left. \frac{e^u (\sin(u) + \cos(u))}{2} \right|_0^{\pi/4} = \frac{e^{\pi/4} (\sin(\pi/4) + \cos(\pi/4))}{2} - \frac{e^0 (\sin(0) + \cos(0))}{2}.
\]

Simplify the trigonometric values:

\[
\sin\left(\frac{\pi}{4}\right) = \cos\left(\frac{\pi}{4}\right) = \frac{\sqrt{2}}{2}, \quad \sin(0) = 0, \quad \cos(0) = 1.
\]

Thus:

\[
\frac{e^{\pi/4} \left( \frac{\sqrt{2}}{2} + \frac{\sqrt{2}}{2} \right)}{2} - \frac{1 \cdot (0 + 1)}{2} = \frac{e^{\pi/4} \sqrt{2}}{2} - \frac{1}{2}.
\]

### Step 5: Final Answer
The exact value of the integral is:

\[
\frac{e^{\pi/4} \sqrt{2} - 1}{2}.
\]

A numerical approximation to 10 decimal places is:

\[
0.7046527126.
\]

### JSON Output
```json
{"answer": "\\frac{\\sqrt{2} e^{\\pi/4} - 1}{2}", "numerical_answer": "0.7046527126"}
```