<think>
Okay, let's tackle this integral step by step. The problem is to compute the definite integral from 0 to 2.0 of ln[(2.0 + sqrt((2.0)^2 - x^2))/x] multiplied by the differential D(0.5x) dx. Hmm, first, I need to make sure I understand the notation here. The D(0.5x) part might be a bit confusing. Wait, in some contexts, D could represent the differential operator, but here it's probably a notation for the differential itself. So, D(0.5x) would be the derivative of 0.5x with respect to x, which is 0.5 dx. So maybe the integral is actually ∫₀² ln[(2 + √(4 - x²))/x] * 0.5 dx. Let me confirm that. If D(0.5x) is the differential, then yes, since d(0.5x) = 0.5 dx. So the integral simplifies to 0.5 times the integral from 0 to 2 of ln[(2 + sqrt(4 - x²))/x] dx. That makes sense.

Alright, so the integral becomes 0.5 * ∫₀² ln[(2 + sqrt(4 - x²))/x] dx. Let me denote the integrand as ln[(2 + sqrt(4 - x²))/x]. Maybe I can simplify the logarithm first. Let's split the logarithm into two terms: ln(2 + sqrt(4 - x²)) - ln(x). So the integral becomes 0.5 [∫₀² ln(2 + sqrt(4 - x²)) dx - ∫₀² ln(x) dx]. That might help break it down.

Let me first compute the second integral, ∫₀² ln(x) dx. The integral of ln(x) dx is x ln(x) - x. Evaluated from 0 to 2. At x=2, it's 2 ln(2) - 2. At x=0, the limit as x approaches 0 of x ln(x) - x is 0 - 0 = 0, since x ln(x) approaches 0. So the second integral is 2 ln(2) - 2. So the second part is straightforward.

Now the first integral is ∫₀² ln(2 + sqrt(4 - x²)) dx. Hmm, this seems trickier. Let me think about substitution. Let me set x = 2 sinθ. Then dx = 2 cosθ dθ. When x=0, θ=0. When x=2, θ=π/2. Let's substitute. The sqrt(4 - x²) becomes sqrt(4 - 4 sin²θ) = 2 cosθ. So the integrand becomes ln(2 + 2 cosθ). So the integral becomes ∫₀^{π/2} ln(2 + 2 cosθ) * 2 cosθ dθ. Wait, no, wait. Wait, x = 2 sinθ, so dx = 2 cosθ dθ. So substituting, the integral becomes:

∫ ln(2 + 2 cosθ) * 2 cosθ dθ from θ=0 to θ=π/2. Wait, no, hold on. Wait, the integrand is ln(2 + sqrt(4 - x²)) dx. After substitution, sqrt(4 - x²) is 2 cosθ, so 2 + sqrt(4 - x²) is 2 + 2 cosθ. So the integrand is ln(2 + 2 cosθ), and dx is 2 cosθ dθ. Therefore, the integral becomes ∫₀^{π/2} ln(2 + 2 cosθ) * 2 cosθ dθ. So that's 2 ∫₀^{π/2} ln(2(1 + cosθ)) cosθ dθ. Let's factor out the 2 inside the log: ln(2) + ln(1 + cosθ). So the integral becomes 2 [ ln(2) ∫₀^{π/2} cosθ dθ + ∫₀^{π/2} ln(1 + cosθ) cosθ dθ ].

Compute the first part: ln(2) ∫₀^{π/2} cosθ dθ = ln(2) [sinθ]₀^{π/2} = ln(2)(1 - 0) = ln(2). So the first term is 2 * ln(2) * 1 = 2 ln(2).

Now the second integral is 2 ∫₀^{π/2} ln(1 + cosθ) cosθ dθ. Hmm, this seems more complicated. Let me denote this integral as I = ∫₀^{π/2} ln(1 + cosθ) cosθ dθ. How can I compute this?

Maybe use integration by parts. Let me set u = ln(1 + cosθ), dv = cosθ dθ. Then du = (-sinθ)/(1 + cosθ) dθ, and v = sinθ. So integration by parts gives uv|₀^{π/2} - ∫₀^{π/2} v du. Let's compute uv: [ln(1 + cosθ) sinθ] from 0 to π/2. At π/2, cosθ = 0, so ln(1 + 0) = ln(1) = 0, so the term is 0. At 0, cosθ = 1, so ln(2) * 0 = 0. So the uv term is 0. Then the integral becomes - ∫₀^{π/2} sinθ * (-sinθ)/(1 + cosθ) dθ = ∫₀^{π/2} (sin²θ)/(1 + cosθ) dθ.

Simplify the integrand: sin²θ/(1 + cosθ). Recall that sin²θ = 1 - cos²θ = (1 - cosθ)(1 + cosθ). So sin²θ/(1 + cosθ) = (1 - cosθ)(1 + cosθ)/(1 + cosθ) = 1 - cosθ. Therefore, the integral becomes ∫₀^{π/2} (1 - cosθ) dθ = [θ - sinθ]₀^{π/2} = (π/2 - 1) - (0 - 0) = π/2 - 1.

So the integral I = ∫₀^{π/2} ln(1 + cosθ) cosθ dθ = π/2 - 1. Therefore, the second term in the original expression is 2*(π/2 - 1) = π - 2.

Putting it all together, the first integral (after substitution) is 2 ln(2) + π - 2. Then the original integral is 0.5 times [ (2 ln(2) + π - 2) - (2 ln(2) - 2) ].

Wait, let's recap. The original integral was 0.5 [ ∫₀² ln(2 + sqrt(4 - x²)) dx - ∫₀² ln(x) dx ].

We computed ∫₀² ln(2 + sqrt(4 - x²)) dx = 2 ln(2) + π - 2.

And ∫₀² ln(x) dx = 2 ln(2) - 2.

So subtracting them: (2 ln(2) + π - 2) - (2 ln(2) - 2) = 2 ln(2) + π - 2 - 2 ln(2) + 2 = π.

Therefore, the original integral is 0.5 * π = π/2.

Wait, that's surprising. So the integral simplifies to π/2. Let me check this again to make sure.

So the first integral after substitution and all steps gives 2 ln(2) + π - 2. The second integral is 2 ln(2) - 2. Subtracting them: (2 ln(2) + π - 2) - (2 ln(2) - 2) = π. Multiply by 0.5: π/2. So the exact answer is π/2. Numerically, π/2 is approximately 1.5707963268. Rounded to 10 decimal places, that's 1.5707963268.

Wait, but let me verify the steps again to be sure. Let's go through the substitution again.

Original integral: 0.5 [ ∫₀² ln(2 + sqrt(4 - x²)) dx - ∫₀² ln(x) dx ]

First integral substitution: x = 2 sinθ, dx = 2 cosθ dθ. Limits from 0 to π/2. Then sqrt(4 - x²) = 2 cosθ. So integrand becomes ln(2 + 2 cosθ). Then the integral becomes ∫₀^{π/2} ln(2 + 2 cosθ) * 2 cosθ dθ. Then split ln(2(1 + cosθ)) into ln2 + ln(1 + cosθ). So the integral becomes 2 [ ln2 ∫ cosθ dθ + ∫ ln(1 + cosθ) cosθ dθ ].

First integral: 2 ln2 [sinθ]₀^{π/2} = 2 ln2 (1 - 0) = 2 ln2.

Second integral: 2 ∫ ln(1 + cosθ) cosθ dθ. Then integration by parts: u = ln(1 + cosθ), dv = cosθ dθ. Then du = -sinθ/(1 + cosθ) dθ, v = sinθ. Then uv term is zero. Then integral becomes ∫ v du = ∫ sinθ * (-sinθ)/(1 + cosθ) dθ. Which is ∫ -sin²θ/(1 + cosθ) dθ. But with a negative sign, so it's ∫ sin²θ/(1 + cosθ) dθ. Then sin²θ = 1 - cos²θ = (1 - cosθ)(1 + cosθ). So sin²θ/(1 + cosθ) = 1 - cosθ. Therefore, the integral becomes ∫ (1 - cosθ) dθ from 0 to π/2. Which is [θ - sinθ] from 0 to π/2: (π/2 - 1) - (0 - 0) = π/2 - 1. Multiply by 2: 2*(π/2 - 1) = π - 2.

So the first integral is 2 ln2 + π - 2. Then the second integral is 2 ln2 - 2. Subtracting them: (2 ln2 + π - 2) - (2 ln2 - 2) = π. Multiply by 0.5: π/2. So yes, the exact answer is π/2. Numerically, π/2 is approximately 1.5707963267948966, so rounded to 10 decimal places, 1.5707963268.

Therefore, the final answer is π/2 with the numerical value as above.
</think>

{"answer": "\\frac{\\pi}{2}", "numerical_answer": "1.5707963268"}