

To solve the definite integral \(\int\limits_0^2 x \arcsin\left(\frac{1}{2} \sqrt{x(2-x)}\right)\,dx\), we proceed as follows:

### Step 1: Simplify the argument of \(\arcsin\)
First, rewrite the expression inside the square root:
\[
x(2-x) = 2x - x^2 = 1 - (x-1)^2
\]
Thus, \(\sqrt{x(2-x)} = \sqrt{1 - (x-1)^2}\), so the integrand becomes:
\[
x \arcsin\left(\frac{1}{2} \sqrt{1 - (x-1)^2}\right)
\]

### Step 2: Substitution \(t = x - 1\)
Let \(t = x - 1\), so \(x = t + 1\) and \(dx = dt\). The limits change from \(x=0\) to \(t=-1\) and \(x=2\) to \(t=1\). The integral becomes:
\[
\int_{-1}^1 (t + 1) \arcsin\left(\frac{1}{2} \sqrt{1 - t^2}\right)\,dt
\]
Split the integral into two parts:
\[
\int_{-1}^1 t \arcsin\left(\frac{1}{2} \sqrt{1 - t^2}\right)\,dt + \int_{-1}^1 \arcsin\left(\frac{1}{2} \sqrt{1 - t^2}\right)\,dt
\]

### Step 3: Odd function cancellation
The first integral involves an odd function (since \(t\) is odd and \(\arcsin\left(\frac{1}{2} \sqrt{1 - t^2}\right)\) is even) over symmetric limits \([-1, 1]\), so it vanishes:
\[
\int_{-1}^1 t \arcsin\left(\frac{1}{2} \sqrt{1 - t^2}\right)\,dt = 0
\]
Thus, the integral reduces to:
\[
\int_{-1}^1 \arcsin\left(\frac{1}{2} \sqrt{1 - t^2}\right)\,dt
\]

### Step 4: Substitution \(t = \sin\theta\)
Let \(t = \sin\theta\), so \(dt = \cos\theta\,d\theta\) and \(\sqrt{1 - t^2} = \cos\theta\). The limits change from \(t=-1\) to \(\theta=-\frac{\pi}{2}\) and \(t=1\) to \(\theta=\frac{\pi}{2}\). The integral becomes:
\[
\int_{-\frac{\pi}{2}}^{\frac{\pi}{2}} \arcsin\left(\frac{1}{2} \cos\theta\right) \cos\theta\,d\theta
\]
Since the integrand is even, we simplify to:
\[
2 \int_{0}^{\frac{\pi}{2}} \arcsin\left(\frac{1}{2} \cos\theta\right) \cos\theta\,d\theta
\]

### Step 5: Integration by parts
Let \(u = \arcsin\left(\frac{1}{2} \cos\theta\right)\) and \(dv = \cos\theta\,d\theta\). Then \(du = \frac{-\frac{1}{2} \sin\theta}{\sqrt{1 - \left(\frac{1}{2} \cos\theta\right)^2}}\,d\theta\) and \(v = \sin\theta\). Integration by parts gives:
\[
uv \bigg|_{0}^{\frac{\pi}{2}} - \int_{0}^{\frac{\pi}{2}} v\,du
\]
The boundary term \(uv\) vanishes at both limits. The remaining integral simplifies to:
\[
\int_{0}^{\frac{\pi}{2}} \frac{\sin^2\theta}{\sqrt{4 - \cos^2\theta}}\,d\theta
\]

### Step 6: Substitution \(u = \cos\theta\)
Let \(u = \cos\theta\), so \(du = -\sin\theta\,d\theta\) and \(\sin^2\theta = 1 - u^2\). The integral becomes:
\[
\int_{0}^{1} \frac{1 - u^2}{\sqrt{4 - u^2}}\,du
\]
Split the integrand:
\[
\int_{0}^{1} \sqrt{4 - u^2}\,du - 3 \int_{0}^{1} \frac{1}{\sqrt{4 - u^2}}\,du
\]

### Step 7: Evaluate the integrals
1. \(\int \sqrt{4 - u^2}\,du = \frac{u}{2}\sqrt{4 - u^2} + 2 \arcsin\left(\frac{u}{2}\right) + C\). Evaluating from \(0\) to \(1\):
\[
\left[\frac{\sqrt{3}}{2} + 2 \cdot \frac{\pi}{6}\right] - 0 = \frac{\sqrt{3}}{2} + \frac{\pi}{3}
\]

2. \(\int \frac{1}{\sqrt{4 - u^2}}\,du = \arcsin\left(\frac{u}{2}\right) + C\). Evaluating from \(0\) to \(1\):
\[
\frac{\pi}{6} - 0 = \frac{\pi}{6}
\]

### Step 8: Combine results
The integral becomes:
\[
\left(\frac{\sqrt{3}}{2} + \frac{\pi}{3}\right) - 3 \cdot \frac{\pi}{6} = \frac{\sqrt{3}}{2} - \frac{\pi}{6}
\]
Multiplying by 2 (from the even function simplification):
\[
2 \left(\frac{\sqrt{3}}{2} - \frac{\pi}{6}\right) = \sqrt{3} - \frac{\pi}{3}
\]

### Numerical Approximation
The exact result is \(\sqrt{3} - \frac{\pi}{3}\). Numerically:
\[
\sqrt{3} \approx 1.73205080757, \quad \frac{\pi}{3} \approx 1.04719755120
\]
Thus:
\[
\sqrt{3} - \frac{\pi}{3} \approx 0.68485325637
\]

{"answer": "\(\sqrt{3} - \frac{\pi}{3}\)", "numerical_answer": "0.6848532564"}