Let's denote the integral as
\[
I_n = \int_0^{\pi/2} \frac{\sin^{2n} x}{\sin^{2n} x + \cos^{2n} x} \, dx
\]

**Step 1. Analytic Solution**

We can use the symmetry of sine and cosine:
Letâ€™s use the substitution \( x \to \frac{\pi}{2} - x \).

Notice that:
\[
\sin\left( \frac{\pi}{2} - x \right) = \cos x,\quad \cos\left( \frac{\pi}{2} - x \right) = \sin x
\]

Consider
\[
I_n' = \int_0^{\pi/2} \frac{\cos^{2n} x}{\cos^{2n} x + \sin^{2n} x} dx
\]
but the integrand is symmetric:
\[
\frac{\sin^{2n} x}{\sin^{2n} x + \cos^{2n} x} + \frac{\cos^{2n} x}{\cos^{2n} x + \sin^{2n} x} = 1
\]
Thus,
\[
I_n + I_n' = \int_0^{\pi/2} 1 dx = \frac{\pi}{2}
\]
But, \( I_n = I_n' \) by the above substitution and the symmetry.

Therefore,
\[
2 I_n = \frac{\pi}{2} \implies I_n = \frac{\pi}{4}
\]
Wait, that would be only if the integral is symmetric, but the integrand is not always symmetric for all \( n \geq 1 \)! That's a mistake. Let's check that:

The function is symmetric if \( n = 1 \), but for \( n > 1 \), let's check if this argument holds.

Actually, from the substitution \( x \to \frac{\pi}{2} - x \):
\[
I_n = \int_0^{\pi/2} \frac{\sin^{2n} x}{\sin^{2n} x + \cos^{2n} x} dx
= \int_0^{\pi/2} \frac{\cos^{2n} x}{\cos^{2n} x + \sin^{2n} x} dx
= \int_0^{\pi/2} \frac{\cos^{2n} x}{\sin^{2n} x + \cos^{2n} x} dx
\]
Therefore,
\[
I_n + I_n = \int_0^{\pi/2} \frac{\sin^{2n} x + \cos^{2n} x}{\sin^{2n} x + \cos^{2n} x} dx = \int_0^{\pi/2} 1 dx = \frac{\pi}{2}
\implies I_n = \frac{\pi}{4}
\]
So regardless of \( n \), for integer \( n \geq 1 \), the value of the integral is always \( \frac{\pi}{4} \).

**Step 2. Numerical Approximation**

\[
\frac{\pi}{4} \approx 0.7853981634
\]

**Final Output (in JSON, rounded to 10 decimal places):**
```json
{"answer": "\\frac{\\pi}{4}", "numerical_answer": "0.7853981634"}
```