<think>
Okay, let's see. I need to compute the definite integral from 0 to infinity of [1/(x(x² + 1²))] * arctan(x/(x² + 1)) dx. Hmm, that looks a bit complicated. Let me break it down step by step.

First, the integrand is a product of two functions: 1/(x(x² + 1)) and arctan(x/(x² + 1)). Maybe substitution could help here. Let me think about possible substitutions. The arctan function's argument is x/(x² + 1). If I let t = x/(x² + 1), maybe? But I'm not sure if that's helpful. Alternatively, perhaps substitution for the entire arctan part. Let me check the derivative of the inside function.

Wait, another approach: sometimes integrals involving arctan can be tackled by integrating by parts. Let's recall that integration by parts formula: ∫u dv = uv - ∫v du. Let me choose u and dv. Let me set u = arctan(x/(x² + 1)), then du would be the derivative of that. Then dv would be the remaining part: 1/(x(x² + 1)) dx. Then I need to compute v by integrating dv. Hmm, integrating 1/(x(x² + 1)) dx. Let me do that first.

To integrate 1/(x(x² + 1)) dx, maybe partial fractions. Let's write 1/(x(x² + 1)) as A/x + (Bx + C)/(x² + 1). Multiply both sides by x(x² + 1):

1 = A(x² + 1) + (Bx + C)x

Expanding the right side: A x² + A + B x² + C x

Combine like terms: (A + B)x² + C x + A

Set coefficients equal on both sides:

For x²: A + B = 0

For x: C = 0

Constant term: A = 1

So from A = 1, then B = -1, and C = 0. Therefore, the partial fractions decomposition is 1/x - x/(x² + 1). Therefore, integrating 1/(x(x² + 1)) dx is ∫(1/x - x/(x² + 1)) dx = ln|x| - (1/2)ln(x² + 1) + C. So that's v.

Wait, but in the integration by parts, dv is 1/(x(x² + 1)) dx, so integrating that gives v = ln x - (1/2) ln(x² + 1). But since we are dealing with definite integrals from 0 to infinity, maybe we need to be careful with the limits. But let's proceed step by step.

So, back to integration by parts. Let me set:

u = arctan(x/(x² + 1))

du/dx = derivative of arctan(u) is 1/(1 + u²) * du/dx. So u = arctan(y), where y = x/(x² + 1). Then du/dx = [1/(1 + y²)] * dy/dx.

Compute dy/dx: y = x/(x² + 1). So dy/dx = [1*(x² + 1) - x*(2x)]/(x² + 1)^2 = [x² + 1 - 2x²]/(x² + 1)^2 = (1 - x²)/(x² + 1)^2.

Therefore, du/dx = [1/(1 + (x²)/(x² + 1)^2)] * (1 - x²)/(x² + 1)^2.

Simplify the denominator: 1 + y² = 1 + [x²/(x² + 1)^2] = [ (x² + 1)^2 + x² ] / (x² + 1)^2.

Wait, let's compute that:

1 + y² = 1 + [x^2 / (x^2 + 1)^2] = [ (x^2 + 1)^2 + x^2 ] / (x^2 + 1)^2.

Expanding numerator: (x^2 + 1)^2 = x^4 + 2x^2 + 1. So numerator is x^4 + 2x^2 + 1 + x^2 = x^4 + 3x^2 + 1.

Therefore, 1 + y² = (x^4 + 3x^2 + 1)/(x^2 + 1)^2.

Therefore, du/dx = [ (1 - x^2)/(x^2 + 1)^2 ] / [ (x^4 + 3x^2 + 1)/(x^2 + 1)^2 ) ] = (1 - x^2)/(x^4 + 3x^2 + 1).

So du = (1 - x^2)/(x^4 + 3x^2 + 1) dx.

Hmm, that seems complicated. Then, the integration by parts formula gives:

∫ u dv = uv | from 0 to ∞ - ∫ v du.

So the original integral is equal to [uv] from 0 to ∞ minus ∫ v du.

But let's compute uv first. uv is [ln x - (1/2) ln(x² + 1)] * arctan(x/(x² + 1)).

But evaluating this from 0 to ∞. Let's check the limits.

As x approaches ∞: arctan(x/(x² + 1)) ≈ arctan(1/x) ≈ 1/x. So as x→infty, arctan term tends to 0. The other part, ln x - (1/2) ln(x² + 1) = ln x - (1/2)(2 ln x + ln(1 + 1/x²)) ) = ln x - ln x - (1/2) ln(1 + 1/x²) ≈ - (1/2)(1/x²) as x→infty. So the product uv tends to 0 * (-0) = 0.

At x=0: arctan(0/(0 + 1)) = arctan(0) = 0. The other part, ln 0 - (1/2) ln(1) = -infty - 0 = -infty. But 0 * (-infty) is an indeterminate form. Hmm, need to check the limit as x approaches 0+.

As x→0+, arctan(x/(x² + 1)) ≈ arctan(x) ≈ x. The other term, ln x - (1/2) ln(x² + 1) ≈ ln x - (1/2)(x²) ≈ ln x. So the product is x * ln x, which tends to 0 (since x approaches 0 and ln x approaches -infty, but x goes to zero faster). So the limit is 0. Therefore, uv evaluated from 0 to ∞ is 0 - 0 = 0.

Therefore, the integral becomes -∫ v du. So the original integral is equal to -∫ from 0 to ∞ of [ln x - (1/2) ln(x² + 1)] * [ (1 - x²)/(x^4 + 3x^2 + 1) ] dx.

Hmm, this seems even more complicated than the original integral. Maybe integration by parts isn't the way to go here. Let me think of another approach.

Alternatively, maybe substitution. Let me consider substitution t = x/(x² + 1). Let's see. Then, t = [ (1)(x² + 1) - x(2x) ] / (x² + 1)^2 dx = [x² + 1 - 2x²]/(x² + 1)^2 dx = (1 - x²)/(x² + 1)^2 dx. Hmm, but in the integrand, we have arctan(t) * [1/(x(x² + 1))] dx. If t = x/(x² + 1), then maybe express the integral in terms of t. Let's see.

But the integrand is arctan(t) * [1/(x(x² + 1))] dx. Let me express x in terms of t. From t = x/(x² + 1), we can write t x² - x + t = 0. Solving for x: quadratic equation t x² - x + t = 0. The solutions are x = [1 ± sqrt(1 - 4t²)]/(2t). Hmm, this might not be straightforward. Maybe this substitution complicates things.

Alternatively, maybe substitution x = tan θ. Let's try that. Let x = tan θ, so θ ∈ [0, π/2) as x goes from 0 to ∞. Then dx = sec² θ dθ. Let's substitute:

Integral becomes ∫_{0}^{π/2} [1/(tan θ (tan² θ + 1))] * arctan( tan θ / (tan² θ + 1) ) * sec² θ dθ.

Simplify tan² θ + 1 = sec² θ, so denominator becomes tan θ * sec² θ. Then 1/(tan θ * sec² θ) * sec² θ dθ = 1/tan θ dθ. So the integral simplifies to ∫_{0}^{π/2} [1/tan θ] * arctan( tan θ / sec² θ ) dθ.

Wait, tan θ / sec² θ = (sin θ / cos θ) / (1 / cos² θ) ) = sin θ cos θ. So arctan(sin θ cos θ). Therefore, the integral becomes ∫_{0}^{π/2} (cot θ) * arctan( (sin θ cos θ) ) dθ.

Hmm, not sure if that's helpful. Let me check if there's a trigonometric identity that can simplify sin θ cos θ. We know that sin(2θ) = 2 sin θ cos θ, so sin θ cos θ = (1/2) sin 2θ. Therefore, arctan( (1/2) sin 2θ ). So the integral is ∫_{0}^{π/2} cot θ * arctan( (1/2) sin 2θ ) dθ.

Still seems complicated. Maybe another substitution. Let me set φ = 2θ. Then when θ = 0, φ = 0; θ = π/2, φ = π. Then dφ = 2 dθ, so dθ = dφ/2. The integral becomes ∫_{0}^{π} (cot(φ/2)) * arctan( (1/2) sin φ ) * (dφ/2).

Hmm, cot(φ/2) is cos(φ/2)/sin(φ/2). Not sure if that helps. Alternatively, maybe another substitution. Let me think.

Alternatively, perhaps differentiation under the integral sign. Let me consider introducing a parameter. Let me define I(a) = ∫_{0}^{∞} [1/(x(x² + 1))] arctan(a x / (x² + 1)) dx. Then our original integral is I(1). Then compute I'(a) and see if that's easier to integrate.

Compute I'(a) = ∫_{0}^{∞} [1/(x(x² + 1))] * [ derivative of arctan(a x / (x² + 1)) w.r. to a ] dx.

Derivative of arctan(u) w.r. to a is [1/(1 + u²)] * (x/(x² + 1)). So I'(a) = ∫_{0}^{∞} [1/(x(x² + 1))] * [ x/(x² + 1) / (1 + (a x / (x² + 1))² ) ] dx.

Simplify the integrand:

[1/(x(x² + 1))] * [x/(x² + 1)] / [1 + (a² x²)/(x² + 1)^2 ] = [1/(x(x² + 1))] * [x/(x² + 1)] / [ ( (x² + 1)^2 + a² x² ) / (x² + 1)^2 ) ]

Simplify numerator and denominator:

= [1/(x(x² + 1))] * [x/(x² + 1)] * [ (x² + 1)^2 / (x^4 + (2 + a²) x² + 1) ) ]

Simplify step by step:

First, 1/(x(x² + 1)) * x/(x² + 1) = 1/(x² + 1)^2.

Then multiplied by (x² + 1)^2 / (x^4 + (2 + a²)x² + 1) = 1 / (x^4 + (2 + a²)x² + 1).

Therefore, I'(a) = ∫_{0}^{∞} 1 / (x^4 + (2 + a²)x² + 1) dx.

Hmm, this seems more manageable. So now, we need to compute I'(a) = ∫_{0}^{∞} dx / (x^4 + (2 + a²)x² + 1). Let's see if we can compute this integral.

The denominator is a quartic polynomial. Let me try to factor it. Let me set y = x². Then the denominator becomes y² + (2 + a²)y + 1. Let's check the discriminant: D = (2 + a²)^2 - 4*1*1 = 4 + 4a² + a^4 - 4 = a^4 + 4a². So sqrt(D) = sqrt(a^4 + 4a²) = a sqrt(a² + 4). Therefore, the roots are y = [ - (2 + a²) ± a sqrt(a² + 4) ] / 2. Hmm, not sure if that's useful. Alternatively, perhaps write the quartic as x^4 + b x² + 1, where b = 2 + a². For such quartics, the integral from 0 to ∞ can be evaluated using substitution or known formulas.

Recall that ∫_{0}^{∞} dx/(x^4 + b x² + 1) = π/(2√(b + 2)) ). Wait, is that a standard integral? Let me verify.

Let me recall that ∫_{0}^{∞ dx/(x^4 + p x² + q) can be evaluated by substitution. Let me try to compute it.

Let me consider the denominator x^4 + b x² + 1. Let me factor it as (x² + m x + 1)(x² - m x + 1). Then expanding, we get x^4 + ( -m² + 2 )x² + 1. Therefore, to match x^4 + b x² + 1, we need -m² + 2 = b => m² = 2 - b. But since b = 2 + a², m² = 2 - (2 + a²) = -a². Which is negative, so this factorization isn't possible. Therefore, maybe another approach.

Alternatively, use substitution x = 1/t. Then, when x approaches 0, t approaches ∞, and vice versa. Then, the integral becomes ∫_{∞}^{0} ( -1/t² ) dt / (1/t^4 + b/t² + 1 ) = ∫_{0}^{∞} t² dt / (1 + b t² + t^4 ). So the integral is equal to ∫_{0}^{∞} t² dt / (t^4 + b t² + 1 ). Adding the original integral and this one, we get ∫_{0}^{∞} (1 + t²)/(t^4 + b t² + 1 ) dt. Let me compute this sum.

Let me denote the original integral as I. Then, I + I = ∫_{0}^{∞} (1 + x²)/(x^4 + b x² + 1 ) dx. Let me compute this integral.

Note that x^4 + b x² + 1 = x^4 + 2 x² + 1 + (b - 2) x² = (x² + 1)^2 + (b - 2)x². Not sure. Alternatively, perhaps write the denominator as x^4 + b x² + 1 = (x² + c x + 1)(x² - c x + 1). Let's try again. Expanding (x² + c x + 1)(x² - c x + 1) = x^4 + (2 - c²) x² + 1. So to get x^4 + b x² + 1, we need 2 - c² = b => c² = 2 - b. But since b = 2 + a², c² = 2 - (2 + a²) = -a². Which is negative, so again, not helpful.

Alternatively, use substitution x = tan θ. Wait, maybe not. Let me try to write the denominator as x^4 + b x² + 1 = x^4 + 2 x² + 1 + (b - 2) x² = (x² + 1)^2 + (b - 2) x². Hmm, not sure.

Alternatively, use substitution t = x - 1/x. Let me try that. Let t = x - 1/x. Then, dt/dx = 1 + 1/x². Hmm, not sure. Alternatively, let me consider the integral I = ∫_{0}^{∞} dx/(x^4 + b x² + 1). Let me split the integral into two parts: from 0 to 1 and from 1 to ∞. In the second part, substitute x = 1/t. Then, ∫_{1}^{∞} dx/(x^4 + b x² + 1) = ∫_{0}^{1} t²/(1 + b t² + t^4 ) dt. So the integral I becomes ∫_{0}^{1} [1/(x^4 + b x² + 1) + x²/(x^4 + b x² + 1)] dx. Which is ∫_{0}^{1} (1 + x²)/(x^4 + b x² + 1) dx. Let me compute this.

The numerator is 1 + x², denominator is x^4 + b x² + 1. Let me divide numerator and denominator by x²: (1/x² + 1)/(x² + b + 1/x²). Let me set t = x + 1/x. Then, t² = x² + 2 + 1/x². So x² + 1/x² = t² - 2. Therefore, denominator becomes t² - 2 + b. The numerator is (1/x² + 1) = (x² + 1)/x². Hmm, not sure. Alternatively, maybe write denominator as x^4 + b x² + 1 = x²(x² + b + 1/x²). Not sure.

Alternatively, let me note that x^4 + b x² + 1 = (x^2 + (b/2))^2 - ( (b^2/4) - 1 ). Hmm, not sure. Alternatively, use substitution y = x^2. Then, dy = 2x dx, so dx = dy/(2√y). Then, the integral becomes ∫_{0}^{∞} 1/(y² + b y + 1) * dy/(2√y). Hmm, not sure.

Wait, maybe use contour integration? But that might be overkill. Alternatively, recall that for integrals of the form ∫_{0}^{∞} dx/(x^4 + p x² + q), there is a standard formula. Let me check.

Yes, the integral ∫_{0}^{∞} dx/(x^4 + p x² + q) can be evaluated by partial fractions or using beta function. Alternatively, using substitution. Let me recall that the integral equals π/(2√(q)) * 1/√(p + 2√q). Wait, not sure. Let me check with specific values. For example, if p = 2 and q = 1, then the integral is ∫_{0}^{∞} dx/(x^4 + 2x² + 1) = ∫_{0}^{∞} dx/(x² + 1)^2 = π/4. On the other hand, if we use the formula π/(2√(q)) * 1/√(p + 2√q)), with q=1, p=2, then it would be π/(2*1) * 1/√(2 + 2*1) = π/2 * 1/√4 = π/2 * 1/2 = π/4. So that works. So the general formula might be ∫_{0}^{∞} dx/(x^4 + p x² + q) = π/(2√q) * 1/√(p + 2√q). Let me verify this.

Let me set x^4 + p x² + q = (x² + a x + b)(x² - a x + b). Then expanding, x^4 + (2b - a²) x² + b². Comparing to x^4 + p x² + q, we have 2b - a² = p and b² = q. So b = √q, and then a² = 2b - p. So if 2b - p ≥ 0, then a = sqrt(2b - p). Then, the integral can be split into partial fractions. But this might not always be possible. However, assuming that the formula holds for positive p and q, then the integral would be π/(2√q) * 1/√(p + 2√q). Let me check with another example. Let p=0, q=1. Then the integral is ∫_{0}^{∞} dx/(x^4 + 1). The standard result is π/(2√2). According to the formula, it's π/(2*1) * 1/√(0 + 2*1) = π/(2) * 1/√2 = π/(2√2), which matches. So the formula seems correct.

Therefore, applying this formula to our case where the denominator is x^4 + (2 + a²)x² + 1. So here, p = 2 + a², q = 1. Then the integral I'(a) = ∫_{0}^{∞} dx/(x^4 + (2 + a²)x² + 1) = π/(2*1) * 1/√( (2 + a²) + 2*1 ) = π/(2) * 1/√(4 + a²).

Therefore, I'(a) = π/(2√(4 + a²)).

Now, we need to integrate I'(a) from a=0 to a=1 to get I(1) - I(0). But wait, originally, we defined I(a) as the integral from 0 to ∞ of [1/(x(x² + 1))] arctan(a x / (x² + 1)) dx. When a=0, arctan(0) = 0, so I(0) = 0. Therefore, I(1) = ∫_{0}^{1} I'(a) da = ∫_{0}^{1} π/(2√(4 + a²)) da.

So compute ∫_{0}^{1} π/(2√(4 + a²)) da. Let's compute this integral.

The integral of 1/√(4 + a²) da is sinh^{-1}(a/2) + C. Alternatively, using substitution. Let me set a = 2 sinh t, then da = 2 cosh t dt. Then √(4 + a²) = √(4 + 4 sinh² t) = 2 cosh t. So the integral becomes ∫ 2 cosh t dt / (2 cosh t) ) = ∫ dt = t + C = sinh^{-1}(a/2) + C. Therefore, the integral from 0 to 1 is sinh^{-1}(1/2) - sinh^{-1}(0). Since sinh^{-1}(0) = 0, and sinh^{-1}(1/2) = ln(1/2 + √(1 + (1/2)^2)) = ln(1/2 + √(5/4)) = ln( (1 + √5)/2 ). Therefore, the integral is π/2 * ln( (1 + √5)/2 ).

Therefore, I(1) = π/2 * ln( (1 + √5)/2 ).

So the exact answer is (π/2) * ln( (1 + √5)/2 ). Let me simplify that expression. Note that (1 + √5)/2 is the golden ratio, often denoted by φ. But we can also rationalize the expression if needed. Alternatively, leave it as is.

Now, compute the numerical approximation. Let's compute (1 + √5)/2 first. √5 ≈ 2.2360679775, so 1 + √5 ≈ 3.2360679775. Divided by 2: ≈ 1.6180339887. Then ln(1.6180339887) ≈ 0.4812118255. Multiply by π/2 ≈ 1.5707963268. So 0.4812118255 * 1.5707963268 ≈ 0.4812118255 * 1.5707963268 ≈ 0.75556... Let me compute this more accurately.

First, compute ln((1 + √5)/2):

(1 + √5)/2 ≈ (1 + 2.2360679775)/2 ≈ 1.61803398875

ln(1.61803398875) ≈ 0.481211825505

π/2 ≈ 1.5707963267948966

Multiply them: 0.481211825505 * 1.5707963267948966 ≈

0.4812118255 * 1.5707963268 ≈

0.4812118255 * 1.5 = 0.4812118255 * 1 = 0.4812118255

0.4812118255 * 0.5707963268 ≈

Let me compute 0.4812118255 * 0.5 = 0.24060591275

0.4812118255 * 0.0707963268 ≈ approx 0.4812118255 * 0.07 = 0.033684827785

Total ≈ 0.24060591275 + 0.033684827785 ≈ 0.2742907405

So total ≈ 0.4812118255 + 0.2742907405 ≈ 0.755502566. So approximately 0.755502566. Rounded to 10 decimal places, let's 0.7555025660. Let me check with a calculator.

Alternatively, use precise calculation:

Compute ln((1 + sqrt(5))/2):

sqrt(5) ≈ 2.23606797749979

(1 + sqrt(5))/2 ≈ (1 + 2.23606797749979)/2 ≈ 3.23606797749979/2 ≈ 1.618033988749895

ln(1.618033988749895) ≈ 0.481211825505059

Multiply by π/2 ≈ 1.5707963267948966:

0.481211825505059 * 1.5707963267948966 ≈

Let me compute this multiplication step by step:

0.481211825505059 * 1.5707963267948966

First, 0.4 * 1.5707963267948966 = 0.6283185307179586

0.08 * 1.5707963267948966 = 0.12566370614359173

0.001211825505059 * 1.5707963267948966 ≈ 0.001211825505059 * 1.5707963268 ≈ 0.0019036539

Adding these together:

0.6283185307179586 + 0.12566370614359173 = 0.7539822368615503

0.7539822368615503 + 0.0019036539 ≈ 0.7558858907615503

Wait, but this seems higher than before. Wait, perhaps I made a mistake in splitting the decimal digits.

Wait, 0.481211825505059 is equal to 0.4 + 0.08 + 0.001211825505059.

But 0.4 * 0.481211825505059 is not 0.4, but the entire number is 0.481211825505059. Wait, no, the number is 0.481211825505059, which is 0.4 + 0.08 + 0.001211825505059. So when multiplying by 1.5707963267948966, we can compute:

0.4 * 1.5707963267948966 = 0.6283185307179586

0.08 * 1.5707963267948966 = 0.12566370614359173

0.001211825505059 * 1.5707963267948966 ≈ 0.001211825505059 * 1.5707963268 ≈ 0.0019036539

Adding these gives 0.6283185307179586 + 0.12566370614359173 = 0.7539822368615503 + 0.0019036539 ≈ 0.7558858907615503. But this contradicts the previous approximate calculation. Hmm, perhaps my initial approximation was wrong.

Wait, use a calculator for precise multiplication:

0.481211825505059 * 1.5707963267948966

Let me compute this:

First, 0.481211825505059 * 1.5707963267948966

Multiply 0.481211825505059 by 1.5707963267948966:

Approximately, 0.4812118255 * 1.5707963268 ≈

Let me compute 0.4812118255 * 1.5707963268:

Breakdown:

0.4 * 1.5707963268 = 0.6283185307

0.08 * 1.5707963268 = 0.1256637061

0.0012118255 * 1.5707963268 ≈ 0.0012118255 * 1.5707963268 ≈ 0.0019036539

Adding these: 0.6283185307 + 0.1256637061 = 0.7539822368 + 0.0019036539 ≈ 0.7558858907.

But this is higher than the previous estimate. Wait, but perhaps the exact value is approximately 0.7558858907. Let me check with a calculator.

Alternatively, use a calculator for exact value:

0.481211825505059 * 1.5707963267948966 ≈

Using a calculator:

0.481211825505059 * 1.5707963267948966 ≈ 0.75556... Wait, perhaps my manual calculation is wrong. Let me use more precise steps.

Alternatively, use the fact that sinh^{-1}(1/2) = ln( (1 + √5)/2 ), and the integral I(1) = π/2 * sinh^{-1}(1/2). So sinh^{-1}(1/2) is approximately 0.4812118255, multiply by π/2 ≈ 1.5707963268, gives 0.4812118255 * 1.5707963268 ≈ 0.75556.

Alternatively, use a calculator for precise value:

Compute 0.481211825505059 * 1.5707963267948966:

0.481211825505059 * 1.5707963267948966 ≈

Let me compute this using more accurate method:

First, write both numbers in decimal:

0.481211825505059

1.5707963267948966

Multiply:

0.481211825505059 * 1.5707963267948966

Multiply 0.481211825505059 by 1.5707963267948966:

First, multiply 0.481211825505059 by 1 = 0.481211825505059

Then, multiply 0.481211825505059 by 0.5707963267948966:

Compute 0.481211825505059 * 0.5 = 0.2406059127525295

0.481211825505059 * 0.0707963267948966 ≈

Compute 0.481211825505059 * 0.07 = 0.03368482778535413

0.481211825505059 * 0.0007963267948966 ≈ 0.481211825505059 * 0.0007963267948966 ≈ approximately 0.0003833

So total for 0.0707963267948966 part: 0.03368482778535413 + 0.0003833 ≈ 0.034068128

So total for 0.5707963267948966 part: 0.2406059127525295 + 0.034068128 ≈ 0.2746740407525295

Therefore, total multiplication: 0.481211825505059 + 0.2746740407525295 ≈ 0.7558858662575885

So approximately 0.7558858662575885. Rounded to 10 decimal places, that's 0.7558858663.

But wait, this contradicts the previous approximate value. Wait, but according to the steps, the exact answer is (π/2) * ln( (1 + √5)/2 ) ≈ 0.7558858663. Let me verify this with a numerical integration of the original integral.

Alternatively, use numerical integration to check. Let me approximate the original integral numerically.

The integral is ∫_{0}^{∞} [1/(x(x² + 1))] arctan(x/(x² + 1)) dx.

Let me make substitution x = tan θ, as before. Then, dx = sec² θ dθ. The integral becomes ∫_{0}^{π/2} [1/(tan θ (tan² θ + 1))] * arctan( tan θ / (tan² θ + 1) ) * sec² θ dθ.

Simplify:

tan² θ + 1 = sec² θ, so denominator becomes tan θ * sec² θ. Then, 1/(tan θ * sec² θ) * sec² θ dθ = 1/tan θ dθ. The integrand becomes (1/tan θ) * arctan( tan θ / sec² θ ) = cot θ * arctan( sin θ cos θ ).

So integral is ∫_{0}^{π/2} cot θ * arctan( sin θ cos θ ) dθ.

Let me compute this numerically. Let's approximate this integral using numerical methods. Let's split the integral into two parts: from 0 to π/4 and π/4 to π/2, to handle possible issues at θ near 0 and π/2.

But for simplicity, use a calculator or approximate using trapezoidal rule.

Alternatively, use substitution. Let t = θ. For θ near 0, cot θ ≈ 1/θ, and sin θ cos θ ≈ θ. So arctan(θ) ≈ θ. So the integrand near 0 is approximately (1/θ) * θ = 1. So the integral near 0 is approximately ∫0^ε 1 dθ = ε, which is finite. Similarly, near π/2, let φ = π/2 - θ. Then cot θ = tan φ ≈ φ. sin θ cos θ = sin(π/2 - φ) cos(π/2 - φ) = cos φ sin φ ≈ φ. So arctan(φ) ≈ φ. So the integrand near π/2 is approximately φ * φ = φ², which is also integrable. Therefore, the integral is convergent.

Let me compute the integral numerically using substitution. Let me use substitution t = sin θ cos θ. Wait, not sure. Alternatively, use numerical approximation.

Alternatively, use a calculator or software. But since I don't do that here, let me use the value we obtained analytically: approximately 0.7558858663. Let me check if this makes sense.

Alternatively, compute the integral numerically using substitution x = t. Let me approximate the integral from 0 to ∞. Let me split it into two parts: from 0 to 1 and from 1 to ∞. For x from 0 to 1, the integrand is [1/(x(x² + 1))] arctan(x/(x² + 1)). For x=0.1: arctan(0.1/(0.01 + 1)) = arctan(0.1/1.01) ≈ 0.0997. The rest is 1/(0.1*(1.01)) ≈ 9.90099. So the integrand at x=0.1 is approx 9.90099 * 0.0997 ≈ 0.987. For x=1: arctan(1/2) ≈ 0.4636, and 1/(1*(1 + 1)) = 0.5. So integrand at x=1 is 0.5 * 0.4636 ≈ 0.2318.

From 1 to ∞, substitute x = 1/t. Then, the integral becomes ∫_{0}^{1} [1/( (1/t)( (1/t²) + 1 )) ] * arctan( (1/t)/( (1/t²) + 1 ) ) * ( -1/t² ) dt. Wait, let me do it properly.

Let x = 1/t, so when x approaches ∞, t approaches 0. Then, dx = -1/t² dt. The integral from 1 to ∞ becomes ∫_{0}^{1} [1/( (1/t)( (1/t²) + 1 )) ] * arctan( (1/t)/( (1/t²) + 1 ) ) * (1/t²) dt.

Simplify the integrand:

1/( (1/t)(1/t² + 1 )) = t / (1/t² + 1) = t / ( (1 + t²)/t² ) ) = t^3 / (1 + t²).

arctan( (1/t)/( (1/t²) + 1 ) ) = arctan( (1/t) / ( (1 + t²)/t² ) ) = arctan( t / (1 + t²) ).

So the integrand becomes [ t^3 / (1 + t²) ] * arctan( t / (1 + t²) ) * (1/t²) dt = [ t / (1 + t²) ] * arctan( t / (1 + t²) ) dt.

Therefore, the integral from 1 to ∞ is equal to ∫_{0}^{1} [ t / (1 + t²) ] * arctan( t / (1 + t²) ) dt.

Therefore, the total integral is ∫_{0}^{1} [1/(x(x² + 1))] arctan(x/(x² + 1)) dx + ∫_{0}^{1} [ t / (1 + t²) ] arctan( t / (1 + t²) ) dt.

But notice that the second integral is the same as the first integral with variable substitution. Let me check:

Let me denote the first integral as I1 = ∫_{0}^{1} [1/(x(x² + 1))] arctan(x/(x² + 1)) dx.

The second integral is I2 = ∫_{0}^{1} [ t / (1 + t²) ] arctan( t / (1 + t²) ) dt.

But if we let u = t in I2, it's the same as I2. So the total integral is I1 + I2. But I1 and I2 are not obviously equal. Wait, but maybe they are equal. Let me check for a specific value. Let t = x. Then I2 is ∫_{0}^{1} [x/(x² + 1)] arctan(x/(x² + 1)) dx. While I1 is ∫_{0}^{1} [1/(x(x² + 1))] arctan(x/(x² + 1)) dx. So they are different. Therefore, the total integral is I1 + I2.

But this doesn't help much. However, since we have an analytical result of approximately 0.7558858663, and the numerical approximation via integrating I'(a) gives the same value, we can trust that the exact answer is (π/2) ln( (1 + √5)/2 ), which is approximately 0.7558858663.

Therefore, the exact answer is (π/2) ln( (1 + √5)/2 ), and the numerical approximation is approximately 0.7558858663, which rounds to 0.7558858663 when rounded to 10 decimal places.

But let me check with another approach. Let me compute the integral numerically using substitution. Let me approximate the integral from 0 to ∞ of [1/(x(x² + 1))] arctan(x/(x² + 1)) dx.

But since I can't compute it here, I'll rely on the analytical result. Therefore, the final answer is π/2 multiplied by the natural logarithm of the golden ratio, which is (1 + √5)/2. So the exact answer is (π/2) * ln( (1 + √5)/2 ), and the numerical value is approximately 0.7558858663.
</think>

{"answer": "\\frac{\\pi}{2} \\ln\\left(\\frac{1 + \\sqrt{5}}{2}\\right)", "numerical_answer": "0.7558858663"}