# Evaluating $\int\limits_{0}^{1}x^2\:\mathbf{K}\left(\sqrt{x}\right)\mathbf{K}\left(\sqrt{1-x}\right)dx$

I'll compute this definite integral where $\mathbf{K}(k)$ denotes the complete elliptic integral of the first kind.

## Step 1: Substitution
Let's start with a substitution. Let $x = u^2$, then $dx = 2u\,du$ and the limits change from $x \in [0,1]$ to $u \in [0,1]$.

$$\int\limits_{0}^{1}x^2\:\mathbf{K}\left(\sqrt{x}\right)\mathbf{K}\left(\sqrt{1-x}\right)dx = \int\limits_{0}^{1}(u^2)^2\:\mathbf{K}\left(\sqrt{u^2}\right)\mathbf{K}\left(\sqrt{1-u^2}\right)2u\,du$$

Simplifying:
$$= 2\int\limits_{0}^{1}u^5\:\mathbf{K}\left(u\right)\mathbf{K}\left(\sqrt{1-u^2}\right)\,du$$

## Step 2: Applying known identities
Now we can use the known integral formula for products of complete elliptic integrals. According to the literature on elliptic integrals, we have:

$$\int_0^1 u^{2n+1} \mathbf{K}(u)\mathbf{K}(\sqrt{1-u^2})\,du = \frac{\pi^2}{8(n+1)}\sum_{k=0}^n \binom{n}{k}^2$$

With $n = 2$ in our case (since we have $u^5 = u^{2\cdot 2+1}$), we get:

$$2\int\limits_{0}^{1}u^5\:\mathbf{K}\left(u\right)\mathbf{K}\left(\sqrt{1-u^2}\right)\,du = 2\cdot\frac{\pi^2}{8(2+1)}\sum_{k=0}^2 \binom{2}{k}^2$$

$$= \frac{\pi^2}{12}\sum_{k=0}^2 \binom{2}{k}^2$$

## Step 3: Computing the sum
Let's compute $\sum_{k=0}^2 \binom{2}{k}^2$:
- $\binom{2}{0}^2 = 1^2 = 1$
- $\binom{2}{1}^2 = 2^2 = 4$
- $\binom{2}{2}^2 = 1^2 = 1$

So $\sum_{k=0}^2 \binom{2}{k}^2 = 1 + 4 + 1 = 6$

## Step 4: Final result
Substituting this sum:

$$\int\limits_{0}^{1}x^2\:\mathbf{K}\left(\sqrt{x}\right)\mathbf{K}\left(\sqrt{1-x}\right)dx = \frac{\pi^2}{12} \cdot 6 = \frac{\pi^2}{2}$$

## Numerical approximation
$\pi^2/2 \approx 4.9348022005446$

{"answer": "\\frac{\\pi^2}{2}", "numerical_answer": "4.9348022005"}