We will show that the integral

  I = ∫₀² x^(1/2) (2 – x)^(–1/2) cosh(√(x(2 – x))) dx

can be written in closed‐form in terms of the modified Bessel function I₀(1). One way to proceed is as follows.

Step 1. Change of variable

A convenient substitution is to set

  x = 1 + cos t,       (1)
   so that 2 – x = 1 – cos t.

When x = 0 we have 0 = 1 + cos t, i.e. cos t = –1 so that t = π; when x = 2 we have 2 = 1 + cos t i.e. cos t = 1 so that t = 0. Also,
  dx/dt = – sin t  ⇒ dx = – sin t dt.

Next note that
  √x = √(1 + cos t) and (2 – x)^(–1/2) = 1/√(1 – cos t).

Using the half–angle formulas
  1 + cos t = 2 cos²(t/2)  and 1 – cos t = 2 sin²(t/2),
we have
  √(1 + cos t) = √2 cos(t/2)  and √(1 – cos t) = √2 sin(t/2).
Thus,
  x^(1/2)(2 – x)^(–1/2) = [√(1 + cos t)]/[√(1 – cos t)] = cos(t/2)/sin(t/2) = cot(t/2).

Also, observe that
  x(2 – x) = (1 + cos t)(1 – cos t) = 1 – cos²t = sin²t,
so that
  √(x(2 – x)) = sin t    (Note: sin t ≥ 0 for t in [0, π]).

Then the integrand becomes
  cot(t/2) cosh(sin t) and dx = – sin t dt.
Thus, changing the limits and absorbing the minus sign we get

  I = ∫₍t=π₎^(t=0) cot(t/2) cosh(sin t) (– sin t dt)
    = ∫₀^(π) cot(t/2) cosh(sin t) sin t dt.

Step 2. A simplification

Write
  cot(t/2) sin t = [cos(t/2)/sin(t/2)] · [2 sin(t/2) cos(t/2)] = 2 cos²(t/2).
Thus, the integral is

  I = ∫₀^(π) 2 cos²(t/2) cosh(sin t) dt.

Now, use the substitution u = t/2. Then du = dt/2, and when t goes from 0 to π, u goes from 0 to π/2. Also, note that
  cos²(t/2) = cos²u  and sin t = sin(2u) = 2 sin u cos u.
Thus,
  I = 2 ∫₀^(π) cos²(t/2) cosh(sin t) dt
    = 2 ∫₀^(π/2) cos²u · cosh(2 sin u cos u) · (2 du)
    = 4 ∫₀^(π/2) cos²u cosh(2 sin u cos u) du.
Since 2 sin u cos u = sin(2u) we may write

  I = 4 ∫₀^(π/2) cos²u cosh(sin(2u)) du.
Now use the double–angle identity for cosine:
  cos²u = (1 + cos 2u)/2.
Thus,

  I = 4 · (1/2) ∫₀^(π/2) [1 + cos 2u] cosh(sin 2u) du
    = 2 ∫₀^(π/2) [1 + cos 2u] cosh(sin 2u) du.
Now, letting v = 2u so that dv = 2 du and when u goes from 0 to π/2, v goes from 0 to π, we obtain

  I = 2 ∫₀^(π) [1 + cos v] cosh(sin v) (dv/2)
    = ∫₀^(π) [1 + cos v] cosh(sin v) dv.
We now split the integral:

  I = ∫₀^(π) cosh(sin v) dv + ∫₀^(π) cos v cosh(sin v) dv.
Notice that the derivative
  d/dv [sinh(sin v)] = cos v cosh(sin v).
Thus,
  ∫₀^(π) cos v cosh(sin v) dv = sinh(sin v) |₀^(π) = sinh(0) – sinh(0) = 0.
Therefore,

  I = ∫₀^(π) cosh(sin v) dv.

Step 3. Recognition of a standard form

It is known that (see, e.g., standard integral tables)
  ∫₀^(π) cosh(a sin θ) dθ = π I₀(a),
so that for a = 1 one has

  I = ∫₀^(π) cosh(sin v) dv = π I₀(1).
Thus we obtain the exact answer

  I = π I₀(1).

Step 4. Numerical Approximation

The modified Bessel function of order zero at 1 is approximately

  I₀(1) ≈ 1.2660658777520082,
so that

  I ≈ π × 1.2660658777520082 ≈ 3.9761170330.

Step 5. Final Answer in JSON format

{"answer": "$\\pi I_0(1)$", "numerical_answer": "3.9761170330"}