To solve the definite integral \(\int_0^1 \frac{x-1}{(x+1)\ln x} \, dx\), we will follow these steps:

### Step 1: Substitution
Let’s make the substitution \(x = e^{-t}\). Then:
- \(dx = -e^{-t} dt\)
- When \(x = 0\), \(t \to \infty\)
- When \(x = 1\), \(t = 0\)
- \(\ln x = -t\)
- The integral becomes:

\[
\int_{\infty}^0 \frac{e^{-t} - 1}{(e^{-t} + 1)(-t)} (-e^{-t}) \, dt = \int_0^{\infty} \frac{e^{-t} - 1}{(e^{-t} + 1)t} e^{-t} \, dt
\]

Simplify the integrand:

\[
\frac{e^{-t} - 1}{(e^{-t} + 1)t} e^{-t} = \frac{(e^{-t} - 1)e^{-t}}{(e^{-t} + 1)t} = \frac{e^{-2t} - e^{-t}}{(e^{-t} + 1)t}
\]

### Step 2: Simplify the Integrand
Divide numerator and denominator by \(e^{-t}\):

\[
\frac{e^{-t} - 1}{1 + e^{t}} \cdot \frac{1}{t} = \frac{e^{-t} - 1}{1 + e^{t}} \cdot \frac{1}{t}
\]

This can be rewritten as:

\[
\frac{e^{-t} - 1}{t(1 + e^{t})} = \frac{1 - e^{t}}{t e^{t}(1 + e^{t})}
\]

But this seems complicated. Let’s try another approach.

### Step 3: Recognize the Integral Form
The integral resembles the form of Frullani integrals or logarithmic integrals. Consider the identity:

\[
\frac{x - 1}{\ln x} = \int_0^1 x^y \, dy
\]

Substitute this into the original integral:

\[
\int_0^1 \frac{x - 1}{(x + 1)\ln x} \, dx = \int_0^1 \frac{1}{x + 1} \left( \int_0^1 x^y \, dy \right) dx = \int_0^1 \int_0^1 \frac{x^y}{x + 1} \, dy \, dx
\]

Swap the order of integration:

\[
\int_0^1 \int_0^1 \frac{x^y}{x + 1} \, dx \, dy
\]

### Step 4: Evaluate the Inner Integral
The inner integral is:

\[
\int_0^1 \frac{x^y}{x + 1} \, dx
\]

This can be expressed in terms of the digamma function \(\psi(y)\). Recall that:

\[
\int_0^1 \frac{x^{y-1}}{x + 1} \, dx = \frac{1}{2} \left( \psi\left(\frac{y + 1}{2}\right) - \psi\left(\frac{y}{2}\right) \right)
\]

For our case, the integral is:

\[
\int_0^1 \frac{x^y}{x + 1} \, dx = \frac{1}{2} \left( \psi\left(\frac{y + 2}{2}\right) - \psi\left(\frac{y + 1}{2}\right) \right)
\]

### Step 5: Integrate with Respect to \(y\)
Now, integrate with respect to \(y\) from 0 to 1:

\[
\int_0^1 \frac{1}{2} \left( \psi\left(\frac{y + 2}{2}\right) - \psi\left(\frac{y + 1}{2}\right) \right) dy
\]

Let \(u = \frac{y + 1}{2}\), then \(du = \frac{dy}{2}\), and the limits change from \(y = 0\) to \(u = \frac{1}{2}\) and \(y = 1\) to \(u = 1\). The integral becomes:

\[
\int_{1/2}^1 \psi(u + \frac{1}{2}) \, du - \int_{1/2}^1 \psi(u) \, du
\]

This can be evaluated using the integral of the digamma function, which is the log-gamma function:

\[
\int \psi(u) \, du = \ln \Gamma(u) + C
\]

Thus:

\[
\left[ \ln \Gamma\left(u + \frac{1}{2}\right) \right]_{1/2}^1 - \left[ \ln \Gamma(u) \right]_{1/2}^1 = \ln \Gamma\left(\frac{3}{2}\right) - \ln \Gamma(1) - \left( \ln \Gamma(1) - \ln \Gamma\left(\frac{1}{2}\right) \right)
\]

Simplify using \(\Gamma(1) = 1\) and \(\Gamma\left(\frac{3}{2}\right) = \frac{1}{2} \Gamma\left(\frac{1}{2}\right) = \frac{\sqrt{\pi}}{2}\):

\[
\ln \left( \frac{\sqrt{\pi}}{2} \right) - \ln 1 - \ln 1 + \ln \left( \sqrt{\pi} \right) = \ln \left( \frac{\sqrt{\pi}}{2} \right) + \ln \left( \sqrt{\pi} \right) = \ln \left( \frac{\pi}{2} \right)
\]

### Step 6: Final Answer
The exact value of the integral is:

\[
\ln \left( \frac{\pi}{2} \right)
\]

Numerical approximation:

\[
\ln \left( \frac{\pi}{2} \right) \approx 0.4515827053
\]

### Final Answer in JSON
```json
{"answer": "\\ln \\left( \\frac{\\pi}{2} \\right)", "numerical_answer": "0.4515827053"}
```