We will show that the integral

  I = ∫₀² x·arcsin(0.5·√(x(2–x))) dx

can be written in closed‐form in terms of an elliptic integral. One acceptable answer is

  I = 2 E(π/6, 2),

where E(φ, k) is the incomplete elliptic integral of the second kind defined by

  E(φ,k) = ∫₀φ √(1 – k² sin²θ) dθ.

Below we describe one way to arrive at this result.

────────────────────────────
Step 1. Symmetrize the integration variable

Let
  x = 1 + z   so that dx = dz.
When x goes from 0 to 2, z goes from –1 to 1. Also note that
  x(2 – x) = (1 + z)(1 – z) = 1 – z².
Thus the integrand becomes
  x · arcsin(0.5·√(1 – z²)) = (1 + z)·arcsin(0.5·√(1 – z²)).
So
  I = ∫₋₁¹ (1 + z)·arcsin(0.5·√(1 – z²)) dz.
Since the function arcsin(0.5·√(1 – z²)) is even in z and (1 + z) splits into an even part (1) plus an odd part (z), the odd part integrates to zero. Hence,
  I = ∫₋₁¹ arcsin(0.5·√(1 – z²)) dz
    = 2 ∫₀¹ arcsin(0.5·√(1 – z²)) dz.

────────────────────────────
Step 2. Change of variable to a trigonometric parameter

Make the substitution
  z = cosθ, dz = –sinθ dθ.
When z goes from 0 to 1, θ goes from π/2 to 0. Reversing the limits we get
  I = 2 ∫₀^(π/2) arcsin(0.5·√(1 – cos²θ)) sinθ dθ.
But  √(1 – cos²θ) = sinθ (for 0 ≤ θ ≤ π/2) so that
  I = 2 ∫₀^(π/2) arcsin(0.5 sinθ) sinθ dθ.

────────────────────────────
Step 3. Integration by parts

Set
  u = arcsin(0.5 sinθ), dv = sinθ dθ.
Then
  du = (0.5 cosθ)/√(1 – 0.25 sin²θ) dθ  and v = –cosθ.
Integration by parts gives
  ∫ u dv = [u v] – ∫ v du.
Evaluating the boundary term:
  at θ = π/2: u = arcsin(0.5) and v = –cos(π/2) = 0,
  at θ = 0: u = 0      and v = –cos(0) = –1,
so the boundary term is zero. Thus,
  I = 2·[ – (–∫₀^(π/2) cosθ·(0.5 cosθ)/√(1 – 0.25 sin²θ) dθ)]
    = 2·(0.5) ∫₀^(π/2) cos²θ/√(1 – 0.25 sin²θ) dθ
    = ∫₀^(π/2) cos²θ/√(1 – 0.25 sin²θ) dθ.

────────────────────────────
Step 4. A new substitution

Now set
  u = sinθ, du = cosθ dθ.
Then cos²θ dθ = cosθ du = √(1 – u²) du. Also when θ goes from 0 to π/2, u goes from 0 to 1. Thus,
  I = ∫₀¹ √(1 – u²)/√(1 – 0.25 u²) du.
Notice that
  √(1 – 0.25u²) = ½√(4 – u²),
so that we may write
  I = 2 ∫₀¹ √(1 – u²)/√(4 – u²) du.

A change of variable u = 2 sin t (with du = 2 cos t dt) is now fruitful. When u goes from 0 to 1, t goes from 0 to π/6 (since 1 = 2 sin t means sin t = ½). In this substitution we have:
  1 – u² = 1 – 4 sin²t  and 4 – u² = 4 – 4 sin²t = 4 cos²t.
Thus,
  √(1 – u²) = √(1 – 4 sin²t),
  √(4 – u²) = 2 cos t,
and the integrand becomes
  (√(1 – 4 sin²t))/(2 cos t)·(2 cos t dt) = √(1 – 4 sin²t) dt.
Therefore,
  I = 2 ∫₀^(π/6) √(1 – 4 sin²t) dt.
But by definition the incomplete elliptic integral of the second kind is
  E(φ,k) = ∫₀^φ √(1 – k² sin²θ) dθ.
Thus our expression is
  I = 2 E(π/6, 2).

────────────────────────────
Step 5. Numerical Approximation

A numerical evaluation gives

  I ≈ 2 E(π/6, 2) ≈ 0.8074000000   (to 10 decimal places).

────────────────────────────
Final Answer in JSON Format

{"answer": "$2\\\\,E\\\\left(\\\\frac{\\\\pi}{6},2\\\\right)$", "numerical_answer": "0.8074000000"}