We wish to evaluate

  I = ∫₀² x^(–1/2) (2–x)^(–1/2) (1+0.5x)^(–2) T₂(√(1+0.5x)) dx.

Step 1. Write the Chebyshev polynomial in closed form.

Recall that the Chebyshev polynomial of the first kind of degree 2 is
  T₂(u) = 2u² – 1.
Thus, with u = √(1+0.5x) we have
  T₂(√(1+0.5x)) = 2(1+0.5x) – 1 = 2 + x – 1 = x + 1.
So the integrand becomes

  f(x) = (x+1) / [√x √(2–x) (1+0.5x)²].

That is,
  I = ∫₀² (x+1) / [√x √(2–x) (1+0.5x)²] dx.

Step 2. Make the substitution x = 2 sin²θ.

Let
  x = 2 sin²θ   with θ ∈ [0, π/2].
Then:
  dx = 4 sinθ cosθ dθ,
  √x = √(2 sin²θ) = √2 sinθ,
  2–x = 2 – 2 sin²θ = 2 cos²θ → √(2–x) = √2 cosθ,
  1+0.5x = 1 + 0.5(2 sin²θ) = 1+ sin²θ,
  x+1 = 2 sin²θ + 1.

Thus, substituting into I we obtain

  I = ∫₀^(π/2) [(2 sin²θ + 1) / ( (√2 sinθ)(√2 cosθ)(1+ sin²θ)² )] (4 sinθ cosθ dθ).

Notice that
  (√2 sinθ)(√2 cosθ) = 2 sinθ cosθ,
so the factors 4 sinθ cosθ/ (2 sinθ cosθ) simplify to 2. Hence

  I = 2 ∫₀^(π/2) (2 sin²θ + 1)/ (1+ sin²θ)² dθ.

Step 3. Write the integrand as a sum of two pieces.

Observe that
  2 sin²θ + 1 = (1 + sin²θ) + sin²θ.
Thus we may write

  I = 2 ∫₀^(π/2) [ (1+ sin²θ)/(1+ sin²θ)² + sin²θ/(1+ sin²θ)² ] dθ
    = 2 ∫₀^(π/2) [ 1/(1+ sin²θ) + sin²θ/(1+ sin²θ)² ] dθ.
Define
  I₁ = ∫₀^(π/2) dθ/(1+ sin²θ)
  I₂ = ∫₀^(π/2) sin²θ/(1+ sin²θ)² dθ.
Then
  I = 2 (I₁ + I₂).

Step 4. Evaluate I₁.

A standard formula is
  ∫₀^(π/2) dθ/(1+ k² sin²θ) = (π/2)/√(1+k²).
For k² = 1 this gives
  I₁ = (π/2)/√2 = π/(2√2).

Step 5. Express I₂ in terms of I₁ and another standard integral.

Write
  sin²θ/(1+ sin²θ)² = 1/(1+ sin²θ) – 1/(1+ sin²θ)².
Thus define
  I₃ = ∫₀^(π/2) dθ/(1+ sin²θ)².
Then
  I₂ = I₁ – I₃.

Step 6. Evaluate I₃.

We now need to compute
  I₃ = ∫₀^(π/2) dθ/(1+ sin²θ)².
A useful method is to change variables with t = tanθ. Then:
  sin²θ = t²/(1+t²),  dθ = dt/(1+t²).
In these terms the denominator becomes
  1 + sin²θ = 1 + t²/(1+t²) = (1+t²+t²)/(1+t²) = (1+2t²)/(1+t²),
so that
  (1+ sin²θ)² = (1+2t²)²/(1+t²)².
Thus,
  I₃ = ∫₀^(∞) [1/(1+t²)] * [(1+t²)²/(1+2t²)²] dt
     = ∫₀^(∞) (1+t²)/(1+2t²)² dt.
Now set u = t√2 so that t = u/√2 and dt = du/√2. Then
  1+t² = 1 + u²/2 = (2+ u²)/2,
  1+2t² = 1+2 (u²/2)= 1+u²,
and therefore
  I₃ = ∫₀^(∞) [(2+ u²)/2] / (1+u²)² · (du/√2)
     = 1/(2√2) ∫₀^(∞) (2+ u²)/(1+u²)² du.
Denote
  J = ∫₀^(∞) (2+ u²)/(1+u²)² du.
This integral splits as
  J = 2∫₀^(∞) du/(1+u²)² + ∫₀^(∞) u² du/(1+u²)².
It is known that
  ∫₀^(∞) du/(1+u²)² = π/4.
Also, note that
  ∫₀^(∞) u² du/(1+u²)² = ∫₀^(∞)[1/(1+u²) – 1/(1+u²)²] du
     = (π/2) – (π/4) = π/4.
Thus,
  J = 2(π/4) + (π/4) = (π/2) + (π/4) = 3π/4.
Returning, we find
  I₃ = 1/(2√2) · (3π/4) = 3π/(8√2).

Step 7. Combine the pieces.

We already had
  I₁ = π/(2√2),
and
  I₂ = I₁ – I₃ = π/(2√2) – 3π/(8√2) = (4π – 3π)/(8√2) = π/(8√2).
Hence,
  I = 2 (I₁ + I₂) = 2 (π/(2√2) + π/(8√2))
     = 2 ((4π + π)/(8√2)) = 2 (5π/(8√2)) = 5π/(4√2).

Step 8. Provide the numerical approximation.

Now, using
  π ≈ 3.141592653589793  and  √2 ≈ 1.414213562373095,
we have:

  I = 5π/(4√2) ≈ (5×3.141592653589793)/(4×1.414213562373095)
       ≈ 15.707963267949/5.65685424949238
       ≈ 2.7768011161.

Thus, the exact value is I = 5π/(4√2) and numerically I ≈ 2.7768011161.

Finally, we output the answer in the required JSON format:

{"answer": "$\\frac{5\\pi}{4\\sqrt{2}}$", "numerical_answer": "2.7768011161"}