

To solve the definite integral \(\int_{-1}^1 \frac{1}{3^x + 1} \, dx\), we use a symmetry argument and substitution.

### Step 1: Define the integral and use substitution
Let \(I = \int_{-1}^1 \frac{1}{3^x + 1} \, dx\). Consider the substitution \(t = -x\), which transforms the integral:
- When \(x = -1\), \(t = 1\); when \(x = 1\), \(t = -1\).
- \(dx = -dt\), so the integral becomes:
  \[
  I = \int_{1}^{-1} \frac{1}{3^{-t} + 1} (-dt) = \int_{-1}^1 \frac{1}{3^{-t} + 1} \, dt
  \]
Renaming \(t\) back to \(x\), we have:
\[
I = \int_{-1}^1 \frac{1}{3^{-x} + 1} \, dx
\]

### Step 2: Simplify the integrand
Note that \(3^{-x} = \frac{1}{3^x}\), so:
\[
\frac{1}{3^{-x} + 1} = \frac{1}{\frac{1}{3^x} + 1} = \frac{3^x}{1 + 3^x}
\]
Thus, \(I = \int_{-1}^1 \frac{3^x}{3^x + 1} \, dx\).

### Step 3: Add the original and transformed integrals
Adding the original \(I\) and the transformed \(I\):
\[
2I = \int_{-1}^1 \left( \frac{1}{3^x + 1} + \frac{3^x}{3^x + 1} \right) dx
\]
The integrand simplifies to:
\[
\frac{1 + 3^x}{3^x + 1} = 1
\]
Thus:
\[
2I = \int_{-1}^1 1 \, dx = 1 - (-1) = 2
\]
Solving for \(I\), we get \(I = 1\).

### Numerical Approximation
The exact value is \(1\), so the numerical approximation to 10 decimal places is \(1.0000000000\).

{"answer": "1", "numerical_answer": "1.0000000000"}