<think>
Okay, let's see. I need to compute the definite integral from 0 to 1 of the fourth root of (1/x - 1) dx. Hmm, the integrand is √[4]{(1/x) - 1}. Let me write that down properly: ∫₀¹ ( (1/x - 1) )^(1/4) dx. 

First, I should check if there are any obvious substitutions or standard integrals that match this form. The expression inside the root is (1/x - 1), which simplifies to (1 - x)/x. So the integrand becomes [(1 - x)/x]^(1/4). That might be a bit tricky. Maybe a substitution to simplify this?

Let me think. If I let t = x/(1 - x), or maybe t = 1/x - 1. Let's try substitution. Let u = 1/x - 1. Then, when x approaches 0, u approaches infinity, and when x approaches 1, u approaches 0. Hmm, but integrating from x=0 to x=1 would translate to u from infinity to 0. That might complicate things. Let's see what du would be.

If u = (1 - x)/x, then x = 1/(u + 1). Then dx = -1/(u + 1)^2 du. So the integral becomes ∫_{u=∞}^{u=0} u^(1/4) * (-1/(u + 1)^2) du. Flipping the limits, that's ∫₀^∞ u^(1/4)/(u + 1)^2 du. Hmm, that seems like a standard integral. Maybe related to the Beta function or Gamma function?

I remember that integrals of the form ∫₀^∞ t^(k - 1)/(1 + t)^(m + n) dt relate to the Beta function B(m, n) when certain conditions are met. Let me recall the Beta function properties. The Beta function is B(p, q) = ∫₀^1 t^(p - 1)(1 - t)^(q - 1) dt, which is also related to Gamma functions: B(p, q) = Γ(p)Γ(q)/Γ(p + q). There's also an integral representation for Beta function from 0 to infinity: B(p, q) = ∫₀^∞ t^(p - 1)/(1 + t)^(p + q) dt. 

Comparing that with my integral ∫₀^∞ u^(1/4)/(u + 1)^2 du. Let me set p - 1 = 1/4, so p = 5/4. Then p + q = 2, so q = 2 - 5/4 = 3/4. Therefore, the integral is B(5/4, 3/4) = Γ(5/4)Γ(3/4)/Γ(2). Since Γ(2) = 1! = 1. So the integral equals Γ(5/4)Γ(3/4).

But I need to compute Γ(5/4) and Γ(3/4). I remember that Γ(1/4) and Γ(3/4) are related through the reflection formula, but maybe there's a way to express Γ(5/4) in terms of Γ(1/4). Let's see. Γ(5/4) = (1/4)Γ(1/4), because Γ(n + 1) = nΓ(n). Similarly, Γ(3/4) is just Γ(3/4). So then, Γ(5/4)Γ(3/4) = (1/4)Γ(1/4)Γ(3/4). 

From the reflection formula, Γ(z)Γ(1 - z) = π / sin(π z). Let's take z = 1/4. Then Γ(1/4)Γ(3/4) = π / sin(π/4) = π / (√2/2) ) = π * 2/√2 = π√2. Therefore, Γ(1/4)Γ(3/4) = π√2. 

So substituting back, Γ(5/4)Γ(3/4) = (1/4) * π√2. Therefore, the integral ∫₀^∞ u^(1/4)/(u + 1)^2 du = π√2 / 4. 

But wait, let me check the substitution steps again to make sure. The original substitution was u = (1 - x)/x, leading to the integral in terms of u. Then, after substitution, the integral became ∫₀^∞ u^(1/4)/(u + 1)^2 du. Then using the Beta function, which gives us Γ(5/4)Γ(3/4)/Γ(2) = Γ(5/4)Γ(3/4). Then using Γ(5/4) = (1/4)Γ(1/4), so Γ(5/4)Γ(3/4) = (1/4)Γ(1/4)Γ(3/4) = (1/4)(π√2). Therefore, the integral is π√2 / 4. 

So the original integral from 0 to 1 of [(1/x - 1)]^(1/4) dx equals π√2 / 4. 

But let me verify this with another substitution to be sure. Alternatively, maybe using a trigonometric substitution. Let me try substituting x = sin²θ or something. Wait, the integrand is (1/x - 1)^(1/4). Let me set x = sin²θ. Then dx = 2 sinθ cosθ dθ. Let's see. When x=0, θ=0; x=1, θ=π/2. Then (1/x -1) = (1/sin²θ -1) = (1 - sin²θ)/sin²θ = cos²θ/sin²θ. So the fourth root of that is (cosθ/sinθ)^(1/2) = sqrt(cotθ). So the integrand becomes sqrt(cotθ) * 2 sinθ cosθ dθ. Let's compute that. 

sqrt(cotθ) is (cosθ/sinθ)^(1/2). Then multiplying by 2 sinθ cosθ gives 2 sinθ cosθ * (cosθ/sinθ)^(1/2) = 2 sinθ cosθ * cos^(1/2)θ / sin^(1/2)θ = 2 sin^(1/2)θ cos^(3/2)θ. So the integral becomes ∫₀^(π/2) 2 sin^(1/2)θ cos^(3/2)θ dθ. 

Hmm, this is similar to the Beta function again. The integral ∫₀^(π/2) sin^mθ cos^nθ dθ = (1/2) B((m +1)/2, (n +1)/2). So here, m = 1/2, n = 3/2. Then the integral is (1/2) B( (1/2 +1)/2, (3/2 +1)/2 ) = (1/2) B(3/4, 5/4). Then B(3/4,5/4) = Γ(3/4)Γ(5/4)/Γ(2) = Γ(3/4)Γ(5/4). Then the integral is (1/2) * Γ(3/4)Γ(5/4). But Γ(5/4) = (1/4)Γ(1/4), so Γ(3/4)Γ(5/4) = (1/4)Γ(1/4)Γ(3/4) = (1/4)π√2) as before. Therefore, the integral becomes (1/2) * (1/4)π√2 = π√2 /8. Wait, but this contradicts the previous result. Wait, but in the substitution here, the integral is 2 times the sin^(1/2)θ cos^(3/2)θ dθ, so the integral is 2 * (1/2) B(3/4,5/4) = B(3/4,5/4). Which is Γ(3/4)Γ(5/4)/Γ(2) = Γ(3/4)Γ(5/4). Which is the same as before. So then, Γ(3/4)Γ(5/4) = (1/4)Γ(1/4)Γ(3/4) = (1/4)π√2). Therefore, the integral is π√2 /4. So both substitutions lead to the same result, which is good. 

Therefore, the exact value is π√2 /4. 

To get the numerical approximation, let's compute π√2 /4. π is approximately 3.1415926536, √2 is approximately 1.4142135624. Multiply them: 3.1415926536 * 1.4142135624 ≈ 4.442882908. Then divide by 4: 4.442882908 /4 ≈ 1.110720727. So approximately 1.110720727. Let me check with a calculator. Alternatively, use more precise values. Let's use more decimal places for π and √2. 

π ≈ 3.141592653589793, √2 ≈ 1.4142135623730951. Multiplying them: 3.141592653589793 * 1.4142135623730951 ≈ 

Let me compute this step by step. 

3.141592653589793 * 1.4142135623730951

First, 3 * 1.4142135623730951 = 4.242640687119285

0.141592653589793 * 1.4142135623730951 ≈ 

0.1 * 1.4142135623730951 = 0.1414213562373095

0.041592653589793 * 1.4142135623730951 ≈ 

0. 0.04 * 1.4142135623730951 = 0.0565685424949238

0.001592653589793 * 1.4142135623730951 ≈ 0.002252

Adding up: 0.1414213562373095 + 0.0565685424949238 ≈ 0.19799, plus 0.002252 ≈ 0.20024. 

So total is 4.242640687119285 + 0.20024 ≈ 4.442880687. So π√2 ≈ 4.442880687. Then divided by 4: 4.442880687 /4 ≈ 1.11072017175. So approximately 1.11072017175. Rounded to 10 decimal places, that's 1.1107201718. Wait, but let me check with a calculator-like approach. Alternatively, use a calculator for π*sqrt(2)/4.

Alternatively, using a calculator, π ≈ 3.141592653589793, sqrt(2) ≈ 1.4142135623730951. So π*sqrt(2) = 3.141592653589793 * 1.4142135623730951 ≈ 4.442882908158366. Then divided by 4: 4.442882908158366 /4 ≈ 1.1107207270395915. So approximately 1.1107207270 when rounded to 10 decimal places. 

Wait, so there's a discrepancy here. Let me check again. Let me compute 3.141592653589793 * 1.4142135623730951:

3 * 1.4142135623730951 = 4.242640687119285

0.141592653589793 * 1.4142135623730951:

Let me compute 0.1 * 1.4142135623730951 = 0.14142135623730951

0.04 * 1.4142135623730951 = 0.056568542494923804

0.001592653589793 * 1.4142135623730951 ≈ 0.001592653589793 * 1.4142135623730951 ≈

First, 0.001 * 1.4142135623730951 ≈ 0.0014142135623730951

0.000592653589793 * 1.4142135623730951 ≈ 0.000592653589793 * 1.4142135623730951 ≈

Approximately 0.000592653589793 * 1.4142135623730951 ≈ 0.000838525

So total for 0.001592653589793 * 1.4142135623730951 ≈ 0.0014142135623730951 + 0.000838525 ≈ 0.002252738

So total for 0.141592653589793 * 0.14142135623730951 + 0.056568542494923804 + 0.002252738 ≈ 0.14142135623730951 + 0.056568542494923804 = 0.19799, plus 0.002252738 ≈ 0.200242738. 

So total π*sqrt(2) ≈ 4.242640687119285 + 0.200242738 ≈ 4.442883425. Then divided by 4: 4.442883425 /4 ≈ 1.11072085625. So approximately 1.1107208563. But this is conflicting with the calculator's exact multiplication. Wait, perhaps my manual calculation is error-prone. Let me use a calculator approach. 

Alternatively, use the fact that π*sqrt(2) ≈ 4.442882908158366. So divided by 4 is approximately 1.1107207270395915. Rounded to 10 decimal places, that's 1.1107207270. 

So the numerical approximation is approximately 1.1107207270. 

Therefore, the exact answer is π√2 /4, and the numerical approximation is approximately 1.1107207270. 

Let me check if there's another way to compute this integral. For example, using substitution t = x, but I think the Beta function approach is solid here. Also, the substitution via trigonometric functions led to the same result, so that's reassuring. 

Another way: Let me check if the integral is a Beta function integral. The original integral from 0 to 1 of [(1/x -1)]^(1/4) dx. Let me make substitution t = x, then when x approaches 0, t approaches 0, but maybe another substitution. Let me set t = 1 - x. Then when x=0, t=1; x=1, t=0. The integral becomes ∫₁⁰ [(1/(1 - t) -1]^(1/4) (-dt). Which is ∫₀¹ [ (1/(1 - t) -1 ) ]^(1/4) dt. Simplify inside: 1/(1 - t) -1 = (1 - (1 - t))/(1 - t) = t/(1 - t). So the integrand becomes (t/(1 - t))^(1/4). So the integral is ∫₀¹ t^(1/4) (1 - t)^(-1/4) dt. Which is the Beta function B(5/4, 3/4). Because Beta function is ∫₀¹ t^{p-1} (1 - t)^{q -1} dt. Here, p -1 = 1/4 ⇒ p = 5/4, and q -1 = -1/4 ⇒ q = 3/4. So B(5/4, 3/4) = Γ(5/4)Γ(3/4)/Γ(2). Since Γ(2) = 1! = 1, so it's Γ(5/4)Γ(3/4). As before, this equals (1/4)Γ(1/4)Γ(3/4) = (1/4)(π√2). So the integral is π√2 /4. 

Therefore, all substitution methods lead to the same result. So the exact answer is π√2 /4. 

So the final answer is π√2 divided by 4, and the numerical value is approximately 1.1107207270. Rounded to 10 decimal places, that's 1.1107207270. 

Let me confirm with a numerical integration. For example, using a calculator or approximate method. Let's take x=0.5. The integrand is (1/0.5 -1)^(1/4) = (2 -1)^(1/4) = 1. At x=0.25, (4 -1)^(1/4) = 3^(1/4) ≈ 1.31607. As x approaches 0, the integrand behaves like (1/x)^(1/4), which is x^(-1/4). The integral of x^(-1/4) from 0 to1 is [x^(3/4)/(3/4)] from 0 to1 = 4/3. So the integral is convergent. The exact value is π√2 /4 ≈ 1.1107, which is less than 4/3 ≈ 1.3333, which makes sense because the integrand is less than x^(-1/4) near 0. So the exact answer seems plausible. 

Therefore, I'm confident that the exact answer is π√2 /4 and the numerical approximation is approximately 1.1107207270.
</think>

{"answer": "\\frac{\\pi \\sqrt{2}}{4}", "numerical_answer": 1.1107207270}