# Evaluating $\int\limits_0^{2.0}x^{-1/4}{(2.0-x)}^{1/4}I_0{(1.0\sqrt[4]{x(2.0-x)})}\:dx$

I'll approach this integral by using a substitution method and recognizing special properties of the modified Bessel function $I_0$.

## Step 1: Substitution
Let's set $u = \sqrt[4]{x(2.0-x)}$, which is symmetric about $x = 1.0$. 

When $x = 0$, $u = 0$
When $x = 2.0$, $u = 0$
When $x = 1.0$, $u = 1.0$ (maximum value)

Due to this symmetry, the function $u(x)$ maps each value of $u$ in $(0,1)$ to two values of $x$, one in $(0,1)$ and one in $(1,2)$.

## Step 2: Transforming the integral

The integrand contains $x^{-1/4}(2.0-x)^{1/4}I_0(1.0\sqrt[4]{x(2.0-x)}) = x^{-1/4}(2.0-x)^{1/4}I_0(1.0u)$

This suggests we should use the properties of $I_0$ and the symmetry of our substitution.

## Step 3: Using properties of modified Bessel functions

For this integral, we can use the result that:

$\int_0^a x^{\nu-1}(a-x)^{\mu-1}I_0(2\sqrt{bx(a-x)})dx = \frac{a^{\nu+\mu-1}}{2^{\nu+\mu-2}}\frac{\Gamma(\nu)\Gamma(\mu)}{\Gamma(\nu+\mu)}I_{\nu-\mu}(ab)$

In our case:
- $a = 2.0$
- $\nu = 3/4$ (since $x^{-1/4} = x^{3/4-1}$)
- $\mu = 5/4$ (since $(2.0-x)^{1/4} = (2.0-x)^{5/4-1}$)
- $b = 1.0/2$ (adjusting for the coefficient in the Bessel function)

## Step 4: Applying the formula

$\int_0^{2.0}x^{-1/4}(2.0-x)^{1/4}I_0(1.0\sqrt[4]{x(2.0-x)})dx = \frac{2.0^{3/4+5/4-1}}{2^{3/4+5/4-2}}\frac{\Gamma(3/4)\Gamma(5/4)}{\Gamma(3/4+5/4)}I_{3/4-5/4}(2.0 \cdot 1.0/2)$

Simplifying:
$= \frac{2.0^{1}}{2^{0}}\frac{\Gamma(3/4)\Gamma(5/4)}{\Gamma(2)}I_{-1/2}(1.0)$

Since $\Gamma(2) = 1!$, and using properties of gamma functions, we can compute:
$\Gamma(3/4)\Gamma(5/4) = \Gamma(3/4)\Gamma(1+1/4) = \Gamma(3/4) \cdot 1/4 \cdot \Gamma(1/4)$

Using the reflection formula $\Gamma(z)\Gamma(1-z) = \frac{\pi}{\sin(\pi z)}$:
$\Gamma(3/4)\Gamma(1/4) = \frac{\pi}{\sin(3\pi/4)} = \frac{\pi}{\sin(\pi/4)} = \frac{\pi}{1/\sqrt{2}} = \pi\sqrt{2}$

Therefore: $\Gamma(3/4)\Gamma(5/4) = \frac{1}{4} \cdot \pi\sqrt{2}$

For the modified Bessel function $I_{-1/2}(1.0)$, we can use the relation $I_{-1/2}(z) = \sqrt{\frac{2}{\pi z}}\cosh(z)$

$I_{-1/2}(1.0) = \sqrt{\frac{2}{\pi \cdot 1.0}}\cosh(1.0) = \sqrt{\frac{2}{\pi}}\cosh(1.0)$

## Step 5: Computing the final result

$\int_0^{2.0}x^{-1/4}(2.0-x)^{1/4}I_0(1.0\sqrt[4]{x(2.0-x)})dx = 2.0 \cdot \frac{1}{4} \cdot \pi\sqrt{2} \cdot \sqrt{\frac{2}{\pi}}\cosh(1.0)$

$= 2.0 \cdot \frac{1}{4} \cdot \pi\sqrt{2} \cdot \frac{\sqrt{2\pi}}{\sqrt{\pi^2}} \cdot \cosh(1.0)$

$= 2.0 \cdot \frac{1}{4} \cdot \sqrt{2} \cdot \sqrt{2} \cdot \cosh(1.0)$

$= 2.0 \cdot \frac{1}{4} \cdot 2 \cdot \cosh(1.0)$

$= 1.0 \cdot \cosh(1.0)$

Calculating $\cosh(1.0) = \frac{e^{1.0} + e^{-1.0}}{2} \approx 1.5430806348$

Therefore, the final result is:
$\int_0^{2.0}x^{-1/4}(2.0-x)^{1/4}I_0(1.0\sqrt[4]{x(2.0-x)})dx = \cosh(1.0)$

## Numerical approximation
$\cosh(1.0) \approx 1.5430806348$

{"answer": "\cosh(1.0)", "numerical_answer": "1.5430806348"}