Let us consider the integral:
\[
I = \int_0^1 \mathbf{K}\left(\sqrt{x}\right)\mathbf{E}\left(\sqrt{1-x}\right)dx
\]

where \(\mathbf{K}(k)\) and \(\mathbf{E}(k)\) are the complete elliptic integrals of the first and second kinds,
\[
\mathbf{K}(k) = \int_0^{\pi/2} \frac{d\theta}{\sqrt{1-k^2 \sin^2\theta}}
\]
\[
\mathbf{E}(k) = \int_0^{\pi/2} \sqrt{1 - k^2 \sin^2\theta} \; d\theta
\]

---

### Step 1: Substitution and Symmetry

Let us try the substitution \(x = \sin^2\theta\), \(dx = 2\sin\theta\cos\theta d\theta = \sin(2\theta) d\theta\), as is often useful for elliptic integrals, with \(x\) running from \(0\) to \(1\), so \(\theta\) runs from \(0\) to \(\frac{\pi}{2}\).

So,
\[
\sqrt{x} = \sin\theta
\]
\[
\sqrt{1-x} = \cos\theta
\]

Then the integral becomes:
\[
I = \int_{\theta=0}^{\pi/2} \mathbf{K}(\sin\theta)\mathbf{E}(\cos\theta) \cdot 2\sin\theta\cos\theta d\theta
\]
\[
= 2 \int_0^{\pi/2} \mathbf{K}(\sin\theta)\mathbf{E}(\cos\theta) \sin\theta \cos\theta d\theta
\]
\[
= \int_0^{\pi/2} \mathbf{K}(\sin\theta)\mathbf{E}(\cos\theta) \sin 2\theta d\theta
\]

---

### Step 2: Consider symmetry and possible alternative forms

Recall a remarkable symmetry for elliptic integrals:

\[
\mathbf{K}(\sin\theta)\mathbf{E}(\cos\theta) + \mathbf{K}(\cos\theta)\mathbf{E}(\sin\theta) = \frac{\pi^2}{4}
\]

Therefore,
\[
\mathbf{K}(\sin\theta)\mathbf{E}(\cos\theta) = \frac{\pi^2}{4} - \mathbf{K}(\cos\theta)\mathbf{E}(\sin\theta)
\]

So the integral becomes:

\[
I = \int_0^{\pi/2} \left( \frac{\pi^2}{4} - \mathbf{K}(\cos\theta)\mathbf{E}(\sin\theta) \right) \sin 2\theta d\theta
\]
\[
= \frac{\pi^2}{4}\int_0^{\pi/2} \sin 2\theta d\theta - \int_0^{\pi/2} \mathbf{K}(\cos\theta)\mathbf{E}(\sin\theta) \sin 2\theta d\theta
\]

But notice that under the change \(\theta \mapsto \frac{\pi}{2} - \theta\), \(\mathbf{K}(\sin\theta)\mathbf{E}(\cos\theta)\) becomes \(\mathbf{K}(\cos\theta)\mathbf{E}(\sin\theta)\), and \(\sin 2\theta\) is unchanged.

So
\[
I = \int_0^{\pi/2} \mathbf{K}(\sin\theta)\mathbf{E}(\cos\theta) \sin 2\theta d\theta = \int_0^{\pi/2} \mathbf{K}(\cos\theta)\mathbf{E}(\sin\theta) \sin 2\theta d\theta
\]

Therefore, the second term is exactly \(I\):
\[
I = \frac{\pi^2}{4} \int_0^{\pi/2} \sin 2\theta d\theta - I
\]
So,
\[
2I = \frac{\pi^2}{4} \int_0^{\pi/2} \sin 2\theta d\theta
\]
\[
I = \frac{\pi^2}{8} \int_0^{\pi/2} \sin 2\theta d\theta
\]
Now, calculate the remaining integral:
\[
\int_0^{\pi/2} \sin 2\theta d\theta = \left. \left( -\frac{1}{2} \cos 2\theta \right) \right|_0^{\pi/2} = -\frac{1}{2} \left[ \cos(\pi) - \cos(0) \right] = -\frac{1}{2} [ -1 - 1 ] = -\frac{1}{2} [-2] = 1
\]

Therefore,
\[
I = \frac{\pi^2}{8} \cdot 1 = \frac{\pi^2}{8}
\]

---

### Step 3: Numerical Value

\[
\frac{\pi^2}{8} \approx \frac{9.869604401}{8} \approx 1.2337005501
\]

---

### Step 4: JSON Output

```json
{"answer": "\\frac{\\pi^2}{8}", "numerical_answer": "1.2337005501"}
```