<think>
Okay, so I need to compute the definite integral from 0 to 1 of ln(x + 1/x) divided by (x + 1/x) dx. Hmm, let's start by simplifying the integrand. The expression x + 1/x can be written as (x² + 1)/x. So the integrand becomes ln((x² + 1)/x) divided by (x² + 1)/x. Let me write that out:

∫₀¹ [ln((x² + 1)/x)] / [(x² + 1)/x] dx

Simplifying the denominator, dividing by (x² + 1)/x is the same as multiplying by x/(x² + 1). So the integrand simplifies to:

ln((x² + 1)/x) * [x/(x² + 1)] dx

Which is:

x * ln((x² + 1)/x) / (x² + 1) dx

Hmm, maybe I can split the logarithm. Let's see, ln((x² + 1)/x) = ln(x² + 1) - ln(x). So substituting that in:

∫₀¹ [x/(x² + 1)] [ln(x² + 1) - ln(x)] dx

So this splits into two integrals:

∫₀¹ [x ln(x² + 1)] / (x² + 1) dx - ∫₀¹ [x ln x] / (x² + 1) dx

Let me handle these two integrals separately. Let's start with the first one: I₁ = ∫ [x ln(x² + 1)] / (x² + 1) dx

Let me make a substitution here. Let u = x² + 1. Then du/dx = 2x, so (du/2) = x dx. Then the integral becomes:

∫ [ln u] / u * (du/2) = (1/2) ∫ (ln u)/u du

The integral of (ln u)/u du is a standard integral. Let me recall that ∫ (ln u)/u du = (ln u)² / 2 + C. So substituting back:

(1/2) * ( (ln u)² / 2 ) + C = (ln u)² / 4 + C

So I₁ evaluated from 0 to 1 would be:

[ (ln(1² + 1))² / 4 - (ln(0² + 1))² / 4 ] = [ (ln 2)² / 4 - (ln 1)² / 4 ] = ( (ln 2)^2 ) / 4 - 0 = (ln 2)^2 / 4

Wait, but wait, when x goes from 0 to 1, u goes from 0² + 1 = 1 to 1² + 1 = 2. So the limits are from u=1 to u=2. So the definite integral I₁ is ( (ln 2)^2 - (ln 1)^2 ) / 4. Since ln 1 = 0, that's (ln 2)^2 / 4. Wait, no, the integral is (1/2) * ( (ln u)^2 / 2 ) evaluated from 1 to 2. Wait, let me check again.

Wait, the integral of (ln u)/u du is (ln u)^2 / 2. So (1/2) times that would be (ln u)^2 / 4. So evaluated from 1 to 2, it's [ (ln 2)^2 / 4 - (ln 1)^2 / 4 ] = (ln 2)^2 / 4. Since ln 1 is 0. So I₁ = (ln 2)^2 / 4.

Okay, that's the first integral. Now the second integral: I₂ = ∫₀¹ [x ln x] / (x² + 1) dx

Hmm, this one might be trickier. Let me think. Let's try substitution. Let u = x² + 1 again. Then du = 2x dx, so x dx = du/2. But then, the integral becomes:

∫ [ln x] / u * (du/2)

But here, x is sqrt(u - 1), so ln x = (1/2) ln(u - 1). So substituting:

(1/2) ∫ [ (1/2) ln(u - 1) ] / u du = (1/4) ∫ ln(u - 1)/u du

Hmm, this seems more complicated. Maybe another substitution. Let me consider integrating from u=1 to u=2, since when x goes from 0 to 1, u goes from 1 to 2. So the integral becomes (1/4) ∫₁² [ln(u - 1)/u] du

Alternatively, maybe integration by parts. Let me try that. Let me set v = ln x, dv = (1/x) dx. Then the other part is x / (x² + 1) dx. Wait, but in I₂, the integrand is x ln x / (x² + 1). So maybe set u_part = ln x, dv_part = x / (x² + 1) dx.

Wait, integration by parts: ∫ u dv = uv - ∫ v du.

Let me set u = ln x, dv = x / (x² + 1) dx

Then du = (1/x) dx, and v = ∫ x / (x² + 1) dx

To compute v, let me substitute w = x² + 1, dw = 2x dx, so (1/2) dw = x dx. Then ∫ x/(x² +1) dx = (1/2) ∫ dw/w = (1/2) ln |w| + C = (1/2) ln(x² +1) + C

So v = (1/2) ln(x² +1)

Therefore, integration by parts gives:

uv | from 0 to 1 - ∫ v du

So:

[ ln x * (1/2) ln(x² +1) ] from 0 to 1 - ∫₀¹ (1/2) ln(x² +1) * (1/x) dx

Hmm, evaluating the first term at x=1: ln(1) * (1/2) ln(2) = 0. At x=0: the limit as x approaches 0+ of ln x * (1/2) ln(x² +1). ln x approaches -infty, but ln(x² +1) approaches ln(1) = 0. So it's 0 * (-infty), which is an indeterminate form. Let's compute the limit:

lim_{x→0+} ln x * (1/2) ln(x² +1) = (1/2) lim_{x→0+} ln x * ln(1 + x²) ≈ (1/2) lim ln x * x² (since ln(1 + x²) ~ x² as x→0). So x² ln x approaches 0, since x² goes to 0 and ln x goes to -infty, but x² dominates. So the limit is 0. Therefore, the first term is 0 - 0 = 0.

So the integral I₂ becomes:

- ∫₀¹ (1/2) ln(x² +1) * (1/x) dx = - (1/2) ∫₀¹ [ln(x² +1)/x] dx

Hmm, this seems challenging. Let me consider substitution here. Let t = x², so when x approaches 0, t approaches 0, and x=1, t=1. Then dt = 2x dx, so x dx = dt/2. But we have 1/x dx. Wait, if t = x², then x = sqrt(t), dx = (1/(2 sqrt(t))) dt. So substituting:

∫ [ln(t +1)/sqrt(t)] * (1/(2 sqrt(t))) dt from t=0 to t=1

Simplify the integrand:

ln(t +1) / sqrt(t) * 1/(2 sqrt(t)) dt = (1/2) ln(t +1) / t dt

So the integral becomes (1/2) ∫₀¹ [ln(t +1)/t] dt

Hmm, this is similar to the dilogarithm function. The integral ∫ ln(1 + t)/t dt from 0 to 1 is known to be π²/12. Wait, let me recall that:

The dilogarithm function Li₂(z) is defined as -∫₀^z [ln(1 - t)/t] dt. But here we have ln(1 + t)/t. Let me check:

If we make substitution u = -t, then ln(1 + t)/t = ln(1 - u)/(-u) = -ln(1 - u)/u. So ∫₀¹ ln(1 + t)/t dt = -∫₀^{-1} ln(1 - u)/u du = -Li₂(-1)

But Li₂(-1) = -π²/12. So -Li₂(-1) = π²/12. Therefore, ∫₀¹ ln(1 + t)/t dt = π²/12

Therefore, the integral (1/2) * π²/12 = π²/24

But wait, let me verify this. Let me recall that:

Li₂(z) = ∑_{n=1}^∞ z^n / n² for |z| ≤ 1. So Li₂(-1) = ∑_{n=1}^∞ (-1)^n / n² = -π²/12. Therefore, ∫₀¹ ln(1 + t)/t dt = -Li₂(-1) = π²/12. So yes, that integral is π²/12. Therefore, the integral (1/2) * π²/12 = π²/24.

Therefore, going back to I₂:

I₂ = - (1/2) * [ π²/24 * 2 ] Wait, wait, let's retrace.

Wait, the original I₂ was:

I₂ = - (1/2) ∫₀¹ [ln(x² +1)/x] dx

Then after substitution, we found that ∫₀¹ [ln(x² +1)/x] dx = (1/2) ∫₀¹ [ln(t +1)/t] dt = (1/2)(π²/12) = π²/24

Therefore, I₂ = - (1/2) * (π²/24) = - π²/48

Wait, no. Wait, the substitution steps:

Original I₂ was:

I₂ = ∫₀¹ [x ln x]/(x² +1) dx

After integration by parts, we had:

I₂ = - (1/2) ∫₀¹ [ln(x² +1)/x] dx

Then we set t = x², so x = sqrt(t), dx = 1/(2 sqrt(t)) dt. Then:

∫₀¹ [ln(x² +1)/x] dx = ∫₀¹ [ln(t +1)/sqrt(t)] * [1/(2 sqrt(t))] dt = (1/2) ∫₀¹ [ln(t +1)/t] dt

Which is (1/2)(π²/12) = π²/24

Therefore, I₂ = - (1/2) * (π²/24) = - π²/48

So putting it all together, the original integral is I₁ - I₂ = ( (ln 2)^2 ) / 4 - ( - π² / 48 )? Wait, no:

Wait, the original integral was I₁ - I₂, where I₁ = (ln 2)^2 / 4 and I₂ = - π² / 48? Wait, no:

Wait, I₁ = (ln 2)^2 / 4

I₂ = - π² / 48

Therefore, the original integral is I₁ - I₂ = (ln 2)^2 / 4 - (- π² / 48) = (ln 2)^2 / 4 + π² / 48

Wait, but let me check again:

Original integral is ∫₀¹ [ln(x + 1/x)] / (x + 1/x) dx = I₁ - I₂, where I₁ = (ln 2)^2 / 4 and I₂ = - π² / 48. So the total integral is (ln 2)^2 / 4 + π² / 48.

Wait, but let me confirm the signs again. The original split was:

∫ [x/(x² +1)] [ln(x² +1) - ln x] dx = I₁ - I₂, where I₁ is the integral of [x ln(x² +1)]/(x² +1) dx and I₂ is the integral of [x ln x]/(x² +1) dx. So yes, the original integral is I₁ - I₂.

We found I₁ = (ln 2)^2 / 4, and I₂ = - π² / 48. Wait, no, in the calculation above, I₂ was found to be - π² / 48. So the original integral is (ln 2)^2 / 4 - ( - π² / 48 ) = (ln 2)^2 / 4 + π² / 48.

Wait, combining these terms. Let me compute the exact value:

( (ln 2)^2 ) / 4 + π² / 48

Is there a way to simplify this further? Let me check if these terms can be combined. Alternatively, perhaps there's a mistake in the calculation. Let me verify each step again.

First, I₁: substitution u = x² +1, leading to (1/2) ∫ (ln u)/u du from u=1 to 2. The integral is (1/2) * [ (ln u)^2 / 2 ] from 1 to 2, which is (1/4)[ (ln 2)^2 - 0 ] = (ln 2)^2 / 4. That's correct.

Then I₂: integration by parts led to - (1/2) ∫ [ln(x² +1)/x] dx. Then substitution t = x², leading to (1/2) ∫ [ln(t +1)/t] dt from 0 to1, which is (1/2)(π²/12) = π²/24. Therefore, I₂ = - (1/2)(π²/24) = - π²/48. Wait, no: the integral after substitution was (1/2)(π²/12) = π²/24. Therefore, I₂ = - (1/2) * (π²/24) = - π²/48. Yes, that's correct.

Therefore, the original integral is I₁ - I₂ = (ln 2)^2 / 4 - ( - π² /48 ) = (ln 2)^2 / 4 + π² /48.

So combining the terms, perhaps we can write this as ( (π²) + 12 (ln 2)^2 ) / 48. Let's check:

(ln 2)^2 /4 is equal to 12 (ln 2)^2 /48, and π² /48 is π² /48. So total is (12 (ln 2)^2 + π² ) /48. So yes, that's a way to write it.

Alternatively, factor out 1/48: (π² + 12 (ln 2)^2 ) / 48.

But maybe there's a more simplified form. Let me check if this is the case.

Alternatively, perhaps there's a mistake in the calculation. Let me check the integral I₂ again.

Wait, when we did the substitution for I₂, we had:

I₂ = ∫₀¹ [x ln x]/(x² +1) dx

Integration by parts: u = ln x, dv = x/(x² +1) dx

Then du = (1/x) dx, v = (1/2) ln(x² +1)

So uv | from 0 to1 is [ln x * (1/2) ln(x² +1)] from 0 to1. At x=1, ln 1 * ... =0. At x=0, the limit as x→0+ of ln x * (1/2) ln(x² +1). As x→0+, ln x → -infty, but ln(x² +1) ~ x², so the product is ln x * x² ~ x² * (-infty), but x² approaches 0. So the limit is 0. Therefore, the first term is 0.

Then the integral becomes - ∫₀¹ v du = - ∫₀¹ (1/2) ln(x² +1) * (1/x) dx

So that's - (1/2) ∫₀¹ [ln(x² +1)/x] dx

Then substitution t = x², so x = sqrt(t), dx = 1/(2 sqrt(t)) dt. Then:

∫₀¹ [ln(x² +1)/x] dx = ∫₀¹ [ln(t +1)/sqrt(t)] * [1/(2 sqrt(t))] dt = (1/2) ∫₀¹ [ln(t +1)/t] dt

Which is (1/2) * ∫₀¹ ln(1 + t)/t dt = (1/2)(π²/12) = π²/24

Therefore, I₂ = - (1/2) * (π²/24) = - π²/48

So that's correct.

Therefore, the original integral is (ln 2)^2 /4 + π² /48

So combining terms:

( (ln 2)^2 * 12 + π² ) / 48

Which is (π² + 12 (ln 2)^2 ) / 48

Alternatively, we can leave it as is. So the exact answer is (ln 2)^2 /4 + π² /48.

Now, let's compute the numerical approximation. Let's compute each term:

First, ln 2 ≈ 0.69314718056

(ln 2)^2 ≈ (0.69314718056)^2 ≈ 0.480453013918

Divided by 4: 0.480453013918 /4 ≈ 0.1201132534795

π² ≈ 9.8696044010893586

π² /48 ≈ 9.8696044010893586 /48 ≈ 0.205616758356

Adding the two terms: 0.1201132534795 + 0.205616758356 ≈ 0.3257300118355

Rounded to 10 decimal places: 0.3257300118

But let me check with more precise calculations.

First, compute ln(2):

ln(2) ≈ 0.69314718055994530941723212145818

(ln(2))^2 ≈ 0.69314718055994530941723212145818^2 ≈ 0.48045301391820142441782711758381

Divide by 4: 0.48045301391820142441782711758381 /4 ≈ 0.12011325347955035610445677939595

π² ≈ 9.8696044010893586188344909998762

π² /48 ≈ 9.8696044010893586188344909998762 /48 ≈ 0.20561675835602830455071856249742

Adding the two:

0.12011325347955035610445677939595 + 0.20561675835602830455071856249742 ≈

0.32573001183557866065517534189337

Rounded to 10 decimal places: 0.3257300118

But let me check with more precise addition:

0.12011325347955035610445677939595

+0.20561675835602830455071856249742

=0.32573001183557866065517534189337

Yes, so approximately 0.3257300118 when rounded to 10 decimal places.

Therefore, the exact answer is (π² + 12 (ln 2)^2 ) /48, and the numerical approximation is approximately 0.3257300118.

But let me check if there's a more simplified form for the exact answer. Let's see:

(π² + 12 (ln 2)^2 ) /48 = π²/48 + (ln 2)^2 /4

Alternatively, factor out 1/12: (π²/4 + 3 (ln 2)^2 ) /12

But I think the form is already simple enough. Alternatively, we can write it as (π² + 12 (ln 2)^2 ) /48.

Alternatively, divide numerator and denominator by 12: (π²/12 + (ln 2)^2 ) /4

But I think the original form is acceptable.

So the exact answer is (π² + 12 (ln 2)^2 ) /48, and the numerical approximation is approximately 0.3257300118.
</think>

{"answer": "\\frac{\\pi^2 + 12 (\\ln 2)^2}{48}", "numerical_answer": 0.3257300118}