# Evaluating $\int_0^1\sqrt[4]{\frac{1}{x}-1}\mathrm{d}x$

I'll evaluate this definite integral analytically and then provide a numerical approximation.

## Step 1: Substitute to simplify the integrand
Let $\frac{1}{x}-1 = t^4$, which means $\frac{1}{x} = 1+t^4$

This gives us $x = \frac{1}{1+t^4}$

Taking the differential:
$dx = -\frac{4t^3}{(1+t^4)^2}dt$

## Step 2: Transform the limits of integration
When $x = 0$: $\frac{1}{x}-1 = \infty$, so $t = \infty$
When $x = 1$: $\frac{1}{x}-1 = 0$, so $t = 0$

## Step 3: Rewrite the integral with the substitution
$\int_0^1\sqrt[4]{\frac{1}{x}-1}\mathrm{d}x = \int_\infty^0 t \cdot \left(-\frac{4t^3}{(1+t^4)^2}\right)dt = \int_0^\infty \frac{4t^4}{(1+t^4)^2}dt$

## Step 4: Use another substitution to simplify further
Let $u = t^4$, then $du = 4t^3dt$, and $t^3dt = \frac{du}{4}$

This gives us:
$\int_0^\infty \frac{4t^4}{(1+t^4)^2}dt = \int_0^\infty \frac{4u}{(1+u)^2} \cdot \frac{1}{4t^3}du = \int_0^\infty \frac{u}{t^3(1+u)^2}du$

Since $u = t^4$, we have $t^3 = \frac{u^{3/4}}{t}$ and $t = u^{1/4}$

Therefore:
$\int_0^\infty \frac{u}{t^3(1+u)^2}du = \int_0^\infty \frac{u}{u^{3/4}(1+u)^2}du = \int_0^\infty \frac{u^{1/4}}{(1+u)^2}du$

## Step 5: Solve using the beta function
This integral can be expressed in terms of the beta function.

Let's use the substitution $v = \frac{1}{1+u}$, which gives $u = \frac{1-v}{v}$ and $du = -\frac{1}{v^2}dv$

When $u = 0$, $v = 1$; when $u = \infty$, $v = 0$

$\int_0^\infty \frac{u^{1/4}}{(1+u)^2}du = \int_1^0 \left(\frac{1-v}{v}\right)^{1/4} \cdot v^2 \cdot \left(-\frac{1}{v^2}\right)dv$
$= \int_0^1 \frac{(1-v)^{1/4}}{v^{1/4}}dv$
$= \int_0^1 (1-v)^{1/4}v^{-1/4}dv$
$= B\left(\frac{5}{4}, \frac{3}{4}\right)$

Where $B(a,b) = \frac{\Gamma(a)\Gamma(b)}{\Gamma(a+b)}$ is the beta function.

## Step 6: Calculate the value using the gamma function
$B\left(\frac{5}{4}, \frac{3}{4}\right) = \frac{\Gamma\left(\frac{5}{4}\right)\Gamma\left(\frac{3}{4}\right)}{\Gamma(2)}$

We know that:
- $\Gamma(2) = 1! = 1$
- $\Gamma\left(\frac{5}{4}\right) = \frac{1}{4}\Gamma\left(\frac{1}{4}\right)$
- $\Gamma\left(\frac{3}{4}\right) = \frac{3}{4}\Gamma\left(-\frac{1}{4}\right)$

Using the reflection formula for the gamma function:
$\Gamma(z)\Gamma(1-z) = \frac{\pi}{\sin(\pi z)}$

With $z = \frac{1}{4}$, we get:
$\Gamma\left(\frac{1}{4}\right)\Gamma\left(\frac{3}{4}\right) = \frac{\pi}{\sin\left(\frac{\pi}{4}\right)} = \frac{\pi}{\frac{1}{\sqrt{2}}} = \pi\sqrt{2}$

Therefore:
$\int_0^1\sqrt[4]{\frac{1}{x}-1}\mathrm{d}x = B\left(\frac{5}{4}, \frac{3}{4}\right) = \frac{\Gamma\left(\frac{5}{4}\right)\Gamma\left(\frac{3}{4}\right)}{\Gamma(2)} = \frac{\pi}{2}$

## Step 7: Numerical approximation
$\frac{\pi}{2} \approx 1.5707963268$

{"answer": "\\frac{\\pi}{2}", "numerical_answer": "1.5707963268"}