Let's evaluate the integral  
\[
I = \int_0^\infty \frac{\{x\}^{\lceil x \rceil}}{1 + \lceil x \rceil} \, dx
\]
where \(\{x\}\) is the fractional part of \(x\), and \(\lceil x \rceil\) is the ceiling function.

### Step 1: Split the Integral over Integers

For \(x \in [n, n+1)\), where \(n\) is a nonnegative integer,
- \(\lceil x \rceil = n+1\),
- \(\{x\} = x - n\).

Thus, over \(x \in [n, n+1)\),
\[
\frac{\{x\}^{\lceil x\rceil}}{1+\lceil x\rceil} = \frac{(x-n)^{n+1}}{n+2}
\]

Thus, 
\[
I = \sum_{n=0}^\infty \int_n^{n+1} \frac{(x-n)^{n+1}}{n+2} \, dx
\]

Let \(t = x-n\), then as \(x\) goes from \(n\) to \(n+1\), \(t\) goes from \(0\) to \(1\):

\[
\int_n^{n+1} (x-n)^{n+1} dx = \int_0^1 t^{n+1} dt = \frac{1}{n+2}
\]

Therefore,
\[
\int_n^{n+1} \frac{(x-n)^{n+1}}{n+2} dx = \frac{1}{n+2} \cdot \frac{1}{n+2} = \frac{1}{(n+2)^2}
\]

### Step 2: Sum Over All \(n\)

\[
I = \sum_{n=0}^{\infty} \frac{1}{(n+2)^2}
\]
Let \(m = n+2\), so as \(n\) goes from \(0\) to \(\infty\), \(m\) goes from \(2\) to \(\infty\):

\[
I = \sum_{m=2}^{\infty} \frac{1}{m^2} = \sum_{m=1}^{\infty} \frac{1}{m^2} - 1
\]
But \(\sum_{m=1}^{\infty} \frac{1}{m^2} = \zeta(2) = \frac{\pi^2}{6}\):

\[
I = \frac{\pi^2}{6} - 1
\]

### Step 3: Numerical Approximation

\[
\frac{\pi^2}{6} \approx 1.644934068
\]
So,
\[
I \approx 1.644934068 - 1 = 0.644934068
\]
Rounded to 10 decimal places: \(0.6449340680\).

---

```json
{"answer": "\\frac{\\pi^2}{6} - 1", "numerical_answer": "0.6449340680"}
```