We start with the integral

  I = ∫₀² x^(–½) (2 – x)^(–½) cos(√(x(2 – x))) dx.

Step 1. Make the substitution x = 2 sin²(t). Then:
  dx = 4 sin(t) cos(t) dt,
  when x = 0 we get t = 0, and when x = 2 we get t = π/2.
Also, we have:
  sin²(t) = x/2 ⇒ √x = √2 sin(t),
  2 – x = 2 cos²(t) ⇒ √(2 – x) = √2 cos(t),
and
  √(x(2 – x)) = √(2 sin²(t) · 2 cos²(t)) = 2 sin(t)cos(t).

The factors in the integrand transform as:
  x^(–½) = 1/(√(2) sin(t)),
  (2 – x)^(–½) = 1/(√(2) cos(t)).
Thus,
  x^(–½)(2 – x)^(–½) = 1/(2 sin(t)cos(t)).

Substitute into the integral:
  I = ∫₀^(π/2) [1/(2 sin(t)cos(t)] cos(2 sin(t)cos(t)) · [4 sin(t)cos(t)] dt
     = 2 ∫₀^(π/2) cos(2 sin(t)cos(t)) dt.

Using the double-angle identity 2 sin(t)cos(t) = sin(2t), we have:
  I = 2 ∫₀^(π/2) cos(sin(2t)) dt.

Step 2. Change variable by letting u = 2t, so du = 2 dt and dt = du/2.
When t = 0, u = 0 and when t = π/2, u = π.
Then,
  I = 2 ∫₀^(π) cos(sin(u)) (du/2) = ∫₀^(π) cos(sin(u)) du.

Step 3. Recognize that the integral
  ∫₀^(π) cos(a sin u) du
has a known result in terms of the Bessel function J₀ when a = 1. In fact, one standard result is:
  ∫₀^(π) cos(sin u) du = π J₀(1).

Thus, the exact answer is:
  I = π J₀(1).

Step 4. Numerical approximation:
The value of the Bessel function J₀(1) is approximately 0.7651976866, so
  I ≈ π × 0.7651976866 ≈ 2.4041138063.

Finally, the answer in the required JSON format is:
{"answer": "$\\pi J_0(1)$", "numerical_answer": "2.4041138063"}