To solve the definite integral \(\int\limits_0^1 \mathbf{K}\left(\sqrt{x}\right)\mathbf{E}\left(\sqrt{1-x}\right)dx\), we need to understand the functions involved. Here, \(\mathbf{K}(k)\) and \(\mathbf{E}(k)\) are the complete elliptic integrals of the first and second kind, respectively.

### Step 1: Analytical Computation

The complete elliptic integrals of the first and second kind are defined as:
\[
\mathbf{K}(k) = \int_0^{\frac{\pi}{2}} \frac{d\theta}{\sqrt{1 - k^2 \sin^2 \theta}}
\]
\[
\mathbf{E}(k) = \int_0^{\frac{\pi}{2}} \sqrt{1 - k^2 \sin^2 \theta} \, d\theta
\]

Given the integral:
\[
\int_0^1 \mathbf{K}\left(\sqrt{x}\right)\mathbf{E}\left(\sqrt{1-x}\right)dx
\]

We can use a known result from the theory of elliptic integrals. Specifically, there is a known result for the product of \(\mathbf{K}(k)\) and \(\mathbf{E}(k')\), where \(k' = \sqrt{1 - k^2}\) is the complementary modulus. The integral can be evaluated using the following identity:
\[
\int_0^1 \mathbf{K}(k) \mathbf{E}(k') \, dk = \frac{\pi}{2}
\]

However, our integral involves \(\mathbf{K}(\sqrt{x})\) and \(\mathbf{E}(\sqrt{1-x})\). To match the form of the known result, we perform a change of variables. Let \(k = \sqrt{x}\), then \(dk = \frac{1}{2\sqrt{x}} dx\), and \(dx = 2k \, dk\). The limits of integration change from \(x = 0\) to \(x = 1\) to \(k = 0\) to \(k = 1\).

Thus, the integral becomes:
\[
\int_0^1 \mathbf{K}(k) \mathbf{E}(\sqrt{1 - k^2}) \cdot 2k \, dk
\]

Using the known result:
\[
\int_0^1 \mathbf{K}(k) \mathbf{E}(\sqrt{1 - k^2}) \, dk = \frac{\pi}{2}
\]

We multiply by 2:
\[
2 \int_0^1 \mathbf{K}(k) \mathbf{E}(\sqrt{1 - k^2}) \, dk = 2 \cdot \frac{\pi}{2} = \pi
\]

### Step 2: Numerical Approximation

To provide a numerical approximation, we can use the value of \(\pi\):
\[
\pi \approx 3.141592653589793
\]

### Step 3: JSON Output

The final answer in the required JSON format is:
```json
{"answer": "\\pi", "numerical_answer": "3.1415926536"}
```