To solve the definite integral \(\int_0^1 \sqrt[3]{x} \left\lfloor \frac{1}{\sqrt[3]{x}} \right\rfloor \, dx\), we need to carefully analyze the integrand and break it down into manageable parts.

### Step 1: Analyze the integrand

The integrand is \(\sqrt[3]{x} \left\lfloor \frac{1}{\sqrt[3]{x}} \right\rfloor\). Let \(y = \sqrt[3]{x}\). Then \(x = y^3\) and \(dx = 3y^2 dy\). The integral becomes:
\[
\int_0^1 y \left\lfloor \frac{1}{y} \right\rfloor 3y^2 \, dy = 3 \int_0^1 y^3 \left\lfloor \frac{1}{y} \right\rfloor \, dy.
\]

### Step 2: Break down the integral

The floor function \(\left\lfloor \frac{1}{y} \right\rfloor\) takes integer values. For \(y\) in the interval \(\left(\frac{1}{n+1}, \frac{1}{n}\right]\), \(\left\lfloor \frac{1}{y} \right\rfloor = n\). Therefore, we can split the integral into a sum of integrals over these intervals:
\[
3 \sum_{n=1}^{\infty} \int_{\frac{1}{n+1}}^{\frac{1}{n}} y^3 n \, dy.
\]

### Step 3: Evaluate each integral

For each \(n\), the integral is:
\[
3n \int_{\frac{1}{n+1}}^{\frac{1}{n}} y^3 \, dy.
\]
The antiderivative of \(y^3\) is \(\frac{y^4}{4}\), so:
\[
3n \left[ \frac{y^4}{4} \right]_{\frac{1}{n+1}}^{\frac{1}{n}} = 3n \left( \frac{\left(\frac{1}{n}\right)^4}{4} - \frac{\left(\frac{1}{n+1}\right)^4}{4} \right) = \frac{3n}{4} \left( \frac{1}{n^4} - \frac{1}{(n+1)^4} \right).
\]
Simplifying, we get:
\[
\frac{3n}{4} \left( \frac{1}{n^4} - \frac{1}{(n+1)^4} \right) = \frac{3}{4} \left( \frac{1}{n^3} - \frac{n}{(n+1)^4} \right).
\]

### Step 4: Sum the series

The integral becomes:
\[
\frac{3}{4} \sum_{n=1}^{\infty} \left( \frac{1}{n^3} - \frac{n}{(n+1)^4} \right).
\]
This can be split into two separate sums:
\[
\frac{3}{4} \left( \sum_{n=1}^{\infty} \frac{1}{n^3} - \sum_{n=1}^{\infty} \frac{n}{(n+1)^4} \right).
\]

The first sum is the Riemann zeta function \(\zeta(3)\):
\[
\sum_{n=1}^{\infty} \frac{1}{n^3} = \zeta(3).
\]

For the second sum, we can reindex \(m = n + 1\):
\[
\sum_{n=1}^{\infty} \frac{n}{(n+1)^4} = \sum_{m=2}^{\infty} \frac{m-1}{m^4} = \sum_{m=2}^{\infty} \left( \frac{1}{m^3} - \frac{1}{m^4} \right).
\]
This can be split into:
\[
\sum_{m=2}^{\infty} \frac{1}{m^3} - \sum_{m=2}^{\infty} \frac{1}{m^4} = \left( \zeta(3) - 1 \right) - \left( \zeta(4) - 1 \right) = \zeta(3) - \zeta(4).
\]

Putting it all together:
\[
\frac{3}{4} \left( \zeta(3) - (\zeta(3) - \zeta(4)) \right) = \frac{3}{4} \zeta(4).
\]

### Step 5: Numerical approximation

The value of \(\zeta(4)\) is \(\frac{\pi^4}{90}\). Therefore:
\[
\frac{3}{4} \zeta(4) = \frac{3}{4} \cdot \frac{\pi^4}{90} = \frac{\pi^4}{120}.
\]

Numerically, \(\pi^4 \approx 97.409091034\), so:
\[
\frac{\pi^4}{120} \approx \frac{97.409091034}{120} \approx 0.811742425.
\]

### Final Answer

\[
\boxed{
\begin{aligned}
\text{"answer": "}\frac{\pi^4}{120}\text{"}, \\
\text{"numerical_answer": "0.811742425"}
\end{aligned}
}
\]