<think>
Okay, so I need to compute the definite integral from 0 to 1 of arctan(sqrt(x(1 - x))) dx. Hmm, let's start by understanding the problem. The integrand is arctan of the square root of x times (1 - x). That square root expression, sqrt(x(1 - x)), looks familiar. It's symmetric around x = 0.5 because if I substitute x with 1 - x, the expression remains the same. Maybe symmetry can help here?

First, let me write down the integral:

I = ∫₀¹ arctan(√(x(1 - x))) dx

I notice that the argument inside the arctan is symmetric. Let me check that. Let’s substitute x with 1 - t. Then when x = 0, t = 1, and x = 1, t = 0. The integral becomes:

I = ∫₁⁰ arctan(√((1 - t)t)) (-dt) = ∫₀¹ arctan(√(t(1 - t))) dt

So, the integral is the same as the original, which confirms the symmetry. Therefore, maybe I can exploit this symmetry by using substitution or expanding the arctan function into a series?

Alternatively, perhaps integration by parts. Let me try that. Let’s set u = arctan(√(x(1 - x))) and dv = dx. Then du would be the derivative of arctan, which is 1/(1 + (sqrt(x(1 - x)))^2) times the derivative of the inside. Let's compute that.

First, let’s compute the derivative of sqrt(x(1 - x)). Let’s denote f(x) = sqrt(x(1 - x)). Then f'(x) = (1/(2sqrt(x(1 - x)))) * (1 - 2x). Therefore, the derivative of arctan(f(x)) is [1/(1 + f(x)^2)] * f'(x). But f(x)^2 is x(1 - x), so 1 + f(x)^2 = 1 + x(1 - x) = 1 + x - x². Therefore, du = [ (1 - 2x)/(2sqrt(x(1 - x))) ] / (1 + x - x²) dx. That seems complicated. Then dv = dx, so v = x. Integration by parts gives:

I = uv|₀¹ - ∫₀¹ v du

But when x approaches 0 or 1, sqrt(x(1 - x)) approaches 0, so arctan(0) is 0. Therefore, uv evaluated at 1 and 0 would be 1*arctan(0) - 0*arctan(0) = 0 - 0 = 0. So the first term is zero, and we have:

I = - ∫₀¹ x * [ (1 - 2x)/(2sqrt(x(1 - x))(1 + x - x²)) ] dx

Hmm, that seems messy. Maybe there's a better substitution. Let me think. Alternatively, perhaps a trigonometric substitution. The expression sqrt(x(1 - x)) is similar to the sine function in a parametrization. Let me try substituting x = sin²θ. Then sqrt(x(1 - x)) would be sinθ cosθ. Let's see:

Let x = sin²θ, so dx = 2 sinθ cosθ dθ. When x = 0, θ = 0; when x = 1, θ = π/2. Then the integral becomes:

I = ∫₀^{π/2} arctan(sinθ cosθ) * 2 sinθ cosθ dθ

But arctan(sinθ cosθ) is arctan( (1/2) sin2θ ). Hmm, not sure if that helps. Alternatively, maybe use substitution t = x - 1/2 to exploit symmetry. Let t = x - 1/2, so x = t + 1/2, dx = dt. The limits become t = -1/2 to t = 1/2. Then the integrand becomes arctan( sqrt( (t + 1/2)(1/2 - t) ) ) = arctan( sqrt( (1/4 - t²) ) )

So sqrt(1/4 - t²) is the expression inside arctan. So the integral becomes:

I = ∫_{-1/2}^{1/2} arctan( sqrt(1/4 - t²) ) dt

But since the integrand is even (symmetric around t=0), we can write:

I = 2 ∫₀^{1/2} arctan( sqrt(1/4 - t²) ) dt

Hmm, maybe another substitution here. Let’s set u = sqrt(1/4 - t²). Then t = sqrt(1/4 - u²). Wait, maybe not. Alternatively, set u = (1/2) sinφ, so that when t = 0, u = 0, and when t = 1/2, u = (1/2) sin(π/2) = 1/2. Wait, maybe not. Alternatively, set t = (1/2) sinφ. Then dt = (1/2) cosφ dφ. Then sqrt(1/4 - t²) = sqrt(1/4 - (1/4) sin²φ) = (1/2) sqrt(1 - sin²φ) = (1/2) cosφ. So the integrand becomes arctan( (1/2) cosφ ). Then the integral becomes:

I = 2 ∫₀^{π/2} arctan( (1/2 cosφ) ) * (1/2 cosφ) dφ

Wait, let me check substitution. If t = (1/2) sinφ, then when t = 0, φ = 0; when t = 1/2, sinφ = 1, so φ = π/2. Then dt = (1/2) cosφ dφ. So substituting into the integral:

I = 2 ∫₀^{π/2} arctan( sqrt(1/4 - (1/2 sinφ)^2 ) ) * (1/2 cosφ) dφ

Wait, but sqrt(1/4 - t²) when t = (1/2) sinφ is sqrt(1/4 - (1/4 sin²φ)) = (1/2) sqrt(1 - sin²φ) = (1/2) cosφ. So the integrand becomes arctan( (1/2 cosφ ). Therefore, the integral becomes:

I = 2 * ∫₀^{π/2} arctan( (1/2 cosφ ) * (1/2 cosφ) dφ )

Wait, no. The original integrand is arctan( sqrt(1/4 - t²) ) dt, and after substitution, sqrt(1/4 - t²) is (1/2 cosφ), and dt is (1/2 cosφ dφ). So the integral becomes:

I = 2 * ∫₀^{π/2} arctan( (1/2 cosφ ) ) * (1/2 cosφ ) dφ

So simplifying:

I = ∫₀^{π/2} arctan( (1/2 cosφ ) ) * cosφ dφ

Hmm, not sure if this is better. Maybe integrating by parts again here. Let’s set u = arctan( (1/2 cosφ ) ), dv = cosφ dφ. Then du = derivative of arctan( (1/2 cosφ ) ) times derivative of (1/2 cosφ ). Let's compute that.

Let’s compute du:

d/dφ [ arctan( (1/2 cosφ ) ) ] = [1 / (1 + ( (1/2 cosφ )^2 ))] * ( -1/2 sinφ )

So du = [ - (1/2 sinφ ) / (1 + (1/4 cos²φ )) ] dφ

And v = sinφ

So integration by parts gives:

uv|₀^{π/2} - ∫₀^{π/2} v du

At φ = π/2, cosφ = 0, so arctan(0) = 0, so uv at π/2 is 0. At φ = 0, sinφ = 0, so uv at 0 is 0. Therefore, the first term is 0. So we have:

I = - ∫₀^{π/2} sinφ * [ - (1/2 sinφ ) / (1 + (1/4 cos²φ )) ] dφ

Simplify:

I = (1/2) ∫₀^{π/2} [ sin²φ / (1 + (1/4 cos²φ )) ] dφ

Simplify denominator:

1 + (1/4 cos²φ ) = (4 + cos²φ ) / 4

So the integral becomes:

I = (1/2) ∫₀^{π/2} [ sin²φ * 4 / (4 + cos²φ ) ] dφ = 2 ∫₀^{π/2} [ sin²φ / (4 + cos²φ ) ] dφ

Hmm, maybe we can simplify this. Let’s write sin²φ as 1 - cos²φ:

I = 2 ∫₀^{π/2} [ (1 - cos²φ ) / (4 + cos²φ ) ] dφ

Let’s split the integral:

I = 2 [ ∫₀^{π/2} 1 / (4 + cos²φ ) dφ - ∫₀^{π/2} cos²φ / (4 + cos²φ ) dφ ]

Let’s compute these two integrals separately. Let’s denote A = ∫₀^{π/2} 1 / (4 + cos²φ ) dφ and B = ∫₀^{π/2} cos²φ / (4 + cos²φ ) dφ. Then I = 2(A - B)

But note that B = ∫₀^{π/2} [ (4 + cos²φ - 4 ) / (4 + cos²φ ) ] dφ = ∫₀^{π/2} [1 - 4/(4 + cos²φ ) ] dφ = (π/2) - 4A

Therefore, substituting back into I:

I = 2(A - (π/2 - 4A)) = 2(5A - π/2) = 10A - π

So now, we need to compute A = ∫₀^{π/2} 1 / (4 + cos²φ ) dφ

To compute A, we can use the standard integral formula for ∫ dx / (a + b cos²x ). The standard technique is to divide numerator and denominator by cos²x, but maybe use substitution. Alternatively, use the identity:

∫₀^{π/2} 1 / (a + b cos²φ ) dφ = π / (2 sqrt(a(a + b)) )

Wait, let me recall the formula. For ∫ dx / (a + b cos²x ) from 0 to π/2, the result is π/(2 sqrt(a(a + b))). Let me verify this.

Let’s set t = tanφ. Then when φ = 0, t = 0; φ = π/2, t approaches infinity. Then cos²φ = 1/(1 + t²), and dφ = dt/(1 + t²). So the integral becomes:

∫₀^∞ [1 / (a + b/(1 + t²)) ] * dt/(1 + t²) = ∫₀^∞ [ (1 + t²) / (a(1 + t²) + b ) ] * dt/(1 + t²) = ∫₀^∞ dt / (a(1 + t²) + b )

= ∫₀^∞ dt / ( (a + b) + a t² )

Which is a standard integral:

∫₀^∞ dx / (c + d x² ) = π/(2 sqrt(c d )) )

So here, c = a + b, d = a. Therefore, the integral is π/(2 sqrt( (a + b) a )) )

Therefore, A = ∫₀^{π/2} 1/(4 + cos²φ ) dφ = π/(2 sqrt(4*(4 + 1)) ) = π/(2 sqrt(20)) ) = π/(2*2*sqrt(5)) ) = π/(4 sqrt(5))

Wait, let's check:

In our case, a = 4, b = 1. So denominator is 4 + cos²φ. Then according to the formula, the integral is π/(2 sqrt(a(a + b)) ) = π/(2 sqrt(4*5)) ) = π/(2*sqrt(20)) = π/(2*2*sqrt(5)) ) = π/(4 sqrt(5))

Yes, correct. Therefore, A = π/(4 sqrt(5))

Then, going back to I = 10A - π = 10*(π/(4 sqrt(5))) - π = (10 π)/(4 sqrt(5)) - π = (5 π)/(2 sqrt(5)) - π = (sqrt(5) π)/2 - π = π ( sqrt(5)/2 - 1 )

Simplify sqrt(5)/2 - 1: Let’s rationalize. sqrt(5)/2 - 1 = (sqrt(5) - 2)/2. Therefore, I = π (sqrt(5) - 2)/2

So the exact answer is (π/2)(sqrt(5) - 2)

Wait, let me check the steps again to make sure.

We had I = 10A - π, where A = π/(4 sqrt(5))

So 10A = 10 * π/(4 sqrt(5)) = (10 π)/(4 sqrt(5)) = (5 π)/(2 sqrt(5)) = (5 π sqrt(5)) / (2*5) ) = (π sqrt(5))/2

Therefore, I = (π sqrt(5))/2 - π = π ( sqrt(5)/2 - 1 )

Which is the same as π ( (sqrt(5) - 2)/2 ) = (π/2)(sqrt(5) - 2)

Yes, that's correct.

So the exact value of the integral is (π/2)(sqrt(5) - 2)

Now, let's compute the numerical approximation. Let's compute sqrt(5) ≈ 2.2360679775

So sqrt(5) - 2 ≈ 0.2360679775

Multiply by π/2: π ≈ 3.1415926536

So π/2 ≈ 1.5707963268

Multiply 0.2360679775 * 1.5707963268 ≈

Let me compute 0.2360679775 * 1.5707963268:

First, 0.2 * 1.5707963268 = 0.31415926536

0.03 * 1.5707963268 = 0.0471238898

0.006 * 1.5707963268 = 0.00942477796

0.0000679775 * 1.5707963268 ≈ approx 0.0001068

Adding up: 0.31415926536 + 0.0471238898 = 0.36128315516

+ 0.00942477796 = 0.37070793312

+ 0.0001068 ≈ 0.37081473312

So approximately 0.37081473312

But let me check with a calculator:

sqrt(5) ≈ 2.2360679775

sqrt(5) - 2 = 0.2360679775

Multiply by π ≈ 0.2360679775 * 3.1415926536 ≈ 0.741539127

Then divide by 2: 0.741539127 / 2 ≈ 0.3707695635

So approximately 0.3707695635. Rounded to 10 decimal places, that would be 0.3707695635. Let me check with a calculator steps:

Alternatively, compute (sqrt(5) - 2) * π / 2:

sqrt(5) ≈ 2.2360679775

sqrt(5) - 2 = 0.2360679775

Multiply by π: 0.2360679775 * 3.141592653589793 ≈ 0.7415391273

Divide by 2: 0.7415391273 / 2 ≈ 0.3707695636

So approximately 0.3707695636. Rounded to 10 decimal places, 0.3707695636.

But let me verify this with a numerical integration to check if this is correct. Let's compute the original integral numerically.

Alternatively, use substitution. Wait, but maybe I made a mistake in the analytical steps. Let me check again.

Wait, when we did the integration by parts, we had I = 10A - π, where A = π/(4 sqrt(5))

So 10A = 10 * π/(4 sqrt(5)) = (5 π)/(2 sqrt(5)) = (π sqrt(5))/2

Therefore, I = (π sqrt(5))/2 - π = π (sqrt(5)/2 - 1 )

Which is equal to π ( (sqrt(5) - 2)/2 )

Yes, that's correct.

So the exact answer is (π/2)(sqrt(5) - 2), and the numerical value is approximately 0.3707695636.

But let me check with a numerical approximation. Let's compute the integral numerically using another method.

Alternatively, use a calculator or numerical integration. For example, using Simpson's rule with several intervals.

But since I can't compute it here step by step, but given that the analytical result gives approximately 0.3707695636, and if I trust the analytical steps, then that's the answer. However, to confirm, let me recall that the integral of arctan(sqrt(x(1 - x))) from 0 to 1 is known? Maybe check if this is a standard integral.

Alternatively, perhaps use substitution t = sqrt(x(1 - x)). Let me try that. Let t = sqrt(x(1 - x)). Then t² = x - x². So x² - x + t² = 0. Solving for x: x = [1 ± sqrt(1 - 4t²)]/2. But this might complicate the substitution. Alternatively, maybe use substitution x = sin²θ, which we tried earlier, but perhaps leads to the same steps.

Alternatively, consider expanding arctan in a power series. Since arctan(z) = ∑_{n=0}^∞ (-1)^n z^{2n+1}/(2n+1) for |z| ≤ 1. Here, the argument inside arctan is sqrt(x(1 - x)), which has a maximum at x=0.5, where it's sqrt(0.25) = 0.5. So the maximum value is 0.5, which is less than 1, so the series converges.

Therefore, we can write:

arctan(sqrt(x(1 - x))) = ∑_{n=0}^∞ (-1)^n [sqrt(x(1 - x))]^{2n+1}/(2n+1) = ∑_{n=0}^∞ (-1)^n (x(1 - x))^{n + 0.5}/(2n+1)

Then integrate term by term from 0 to 1:

I = ∑_{n=0}^∞ [ (-1)^n / (2n+1) ] ∫₀¹ (x(1 - x))^{n + 0.5} dx

The integral ∫₀¹ x^{n + 0.5} (1 - x)^{n + 0.5} dx is the Beta function B(n + 1.5, n + 1.5) = Γ(n + 1.5)^2 / Γ(2n + 3)

But Γ(n + 1.5) = (n + 0.5)(n - 0.5)...0.5 sqrt(π) by the property of Gamma function. Alternatively, using the duplication formula.

But Beta function B(a, a) = 2^{1 - 2a} sqrt(π) Γ(a) / Γ(a + 0.5). Wait, but here a = n + 1.5. Hmm, maybe not directly helpful.

Alternatively, express the integral in terms of factorials. Since for integer n, B(n + 1.5, n + 1.5) = (Γ(n + 1.5))^2 / Γ(2n + 3). But Γ(n + 1.5) = (n + 0.5)(n - 0.5)...0.5 sqrt(π). So:

Γ(n + 1.5) = (sqrt(π)/2^{2n + 1}) ) (2n + 1)! ) / n! )

Wait, perhaps not. Let me recall that Γ(n + 1/2) = (2n)! sqrt(π) / (4^n n! )

But here we have Γ(n + 1.5) = Γ(n + 1 + 0.5) = (n + 0.5) Γ(n + 0.5) = (n + 0.5)(n - 0.5)...0.5 sqrt(π)

Alternatively, using the duplication formula:

Γ(z)Γ(z + 0.5) = 2^{1 - 2z} sqrt(π) Γ(2z)

But I might be getting stuck here. Alternatively, compute the integral ∫₀¹ x^{n + 0.5} (1 - x)^{n + 0.5} dx = B(n + 1.5, n + 1.5) = [Γ(n + 1.5)]^2 / Γ(2n + 3)

But Γ(n + 1.5) = (n + 0.5)(n - 0.5)...0.5 sqrt(π) = sqrt(π) * ( (2n + 1)!! ) / 2^{n + 1} )

Wait, the double factorial for odd numbers: (2n + 1)!! = (2n + 1)(2n - 1)...3*1

But Γ(n + 1.5) = (2n + 1)!! sqrt(π) / 2^{n + 1}

Therefore, [Γ(n + 1.5)]^2 = π ( (2n + 1)!! )^2 / 2^{2n + 2}

And Γ(2n + 3) = (2n + 2)! / 2^{2n + 2} (using Γ(m) = (m - 1)! for integer m)

Wait, no. Γ(2n + 3) = (2n + 2)!.

Therefore, B(n + 1.5, n + 1.5) = [Γ(n + 1.5)]^2 / Γ(2n + 3) = [ π ( (2n + 1)!! )^2 / 2^{2n + 2} ] / (2n + 2)! )

But (2n + 2)! = (2n + 2)(2n + 1)!! * 2^{n + 1} (n + 1)! )

Wait, perhaps this is getting too complicated. Alternatively, use the Beta function relation to the binomial coefficients.

Alternatively, perhaps use the substitution x = sin²θ again. Then the integral becomes:

∫₀^{π/2} (sin²θ)^{n + 0.5} (cos²θ)^{n + 0.5} * 2 sinθ cosθ dθ

= 2 ∫₀^{π/2} sin^{2n + 2}θ cos^{2n + 2}θ dθ

= 2 * (1/2) B(n + 1.5, n + 1.5) = B(n + 1.5, n + 1.5)

Which is the previous result. So this doesn't help.

Alternatively, use the formula for the Beta function in terms of factorials for half-integers. But I think this might not be the best approach. Given that we already have an analytical result, perhaps it's better to proceed with that.

Therefore, the exact answer is (π/2)(sqrt(5) - 2), and the numerical approximation is approximately 0.3707695636. Rounded to 10 decimal places, that's 0.3707695636.

But let me check with a calculator. Let's compute (sqrt(5) - 2) * π / 2:

sqrt(5) ≈ 2.2360679775

sqrt(5) - 2 = 0.2360679775

Multiply by π ≈ 3.141592653589793:

0.2360679775 * 3.141592653589793 ≈ 0.7415391273

Divide by 2: 0.7415391273 / 2 ≈ 0.3707695636

Yes, so the numerical value is approximately 0.3707695636. Rounded to 10 decimal places, it's 0.3707695636.

Therefore, the final answer is:

Exact: (π/2)(√5 - 2)

Numerical: 0.3707695636
</think>

{"answer": "\\frac{\\pi}{2}(\\sqrt{5} - 2)", "numerical_answer": "0.3707695636"}