

To solve the definite integral \(\int_0^{\frac{\pi}{4}}\tan^{-1}\left(\frac{1+\tan(x)}{\sqrt{2}}\right)\mathrm{d}x\), we proceed as follows:

### Step 1: Substitution and Symmetry
Let \(I = \int_0^{\frac{\pi}{4}}\tan^{-1}\left(\frac{1+\tan(x)}{\sqrt{2}}\right)\mathrm{d}x\). Consider the substitution \(t = \frac{\pi}{4} - x\), which transforms the integral limits: when \(x = 0\), \(t = \frac{\pi}{4}\); when \(x = \frac{\pi}{4}\), \(t = 0\). The differential becomes \(\mathrm{d}x = -\mathrm{d}t\), so:
\[
I = \int_{\frac{\pi}{4}}^0 \tan^{-1}\left(\frac{1+\tan\left(\frac{\pi}{4} - t\right)}{\sqrt{2}}\right) (-\mathrm{d}t) = \int_0^{\frac{\pi}{4}} \tan^{-1}\left(\frac{1+\tan\left(\frac{\pi}{4} - t\right)}{\sqrt{2}}\right) \mathrm{d}t.
\]

### Step 2: Simplify \(\tan\left(\frac{\pi}{4} - t\right)\)
Using the tangent subtraction formula \(\tan(A - B) = \frac{\tan A - \tan B}{1 + \tan A \tan B}\), we have:
\[
\tan\left(\frac{\pi}{4} - t\right) = \frac{1 - \tan t}{1 + \tan t}.
\]
Thus:
\[
1 + \tan\left(\frac{\pi}{4} - t\right) = 1 + \frac{1 - \tan t}{1 + \tan t} = \frac{(1 + \tan t) + (1 - \tan t)}{1 + \tan t} = \frac{2}{1 + \tan t}.
\]
Substituting back, the argument of \(\tan^{-1}\) becomes:
\[
\frac{1+\tan\left(\frac{\pi}{4} - t\right)}{\sqrt{2}} = \frac{2}{\sqrt{2}(1 + \tan t)} = \frac{\sqrt{2}}{1 + \tan t}.
\]
Thus, the integral in terms of \(t\) is:
\[
I = \int_0^{\frac{\pi}{4}} \tan^{-1}\left(\frac{\sqrt{2}}{1 + \tan t}\right) \mathrm{d}t.
\]

### Step 3: Combine Integrals
Adding the original integral \(I\) and the transformed integral, we get:
\[
2I = \int_0^{\frac{\pi}{4}} \left[ \tan^{-1}\left(\frac{1+\tan x}{\sqrt{2}}\right) + \tan^{-1}\left(\frac{\sqrt{2}}{1 + \tan x}\right) \right] \mathrm{d}x.
\]
For \(z > 0\), \(\tan^{-1}(z) + \tan^{-1}\left(\frac{1}{z}\right) = \frac{\pi}{2}\). Here, \(z = \frac{1+\tan x}{\sqrt{2}} > 0\), so:
\[
\tan^{-1}\left(\frac{1+\tan x}{\sqrt{2}}\right) + \tan^{-1}\left(\frac{\sqrt{2}}{1 + \tan x}\right) = \frac{\pi}{2}.
\]
Thus:
\[
2I = \int_0^{\frac{\pi}{4}} \frac{\pi}{2} \mathrm{d}x = \frac{\pi}{2} \cdot \frac{\pi}{4} = \frac{\pi^2}{8}.
\]
Therefore, \(I = \frac{\pi^2}{16}\).

### Numerical Approximation
The numerical value of \(\frac{\pi^2}{16}\) is approximately \(0.6168502755\) (rounded to 10 decimal places).

{"answer": "\(\frac{\pi^2}{16}\)", "numerical_answer": "0.6168502755"}