<think>
Okay, let's see. I need to compute the definite integral of 1/(1 - x²) from -1/2 to 1/2. Hmm, first, I remember that the integral of 1/(1 - x²) dx is a standard integral. Wait, isn't that related to inverse hyperbolic functions or maybe logarithmic functions? Let me think. The integral of 1/(1 - x²) can be expressed using partial fractions. Right, because 1/(1 - x²) can be written as A/(1 - x) + B/(1 + x). Let me check that.

So, 1/(1 - x²) = A/(1 - x) + B/(1 + x). Multiplying both sides by (1 - x)(1 + x) gives 1 = A(1 + x) + B(1 - x). To find A and B, I can set up equations by choosing suitable values for x. Let me set x = 1: 1 = A(2) + B(0) => A = 1/2. Similarly, set x = -1: 1 = A(0) + B(2) => B = 1/2. So, the integral becomes the integral from -1/2 to 1/2 of [1/(2(1 - x)) + 1/(2(1 + x))] dx.

Now, integrating term by term. The integral of 1/(1 - x) dx is -ln|1 - x| + C, and the integral of 1/(1 + x) dx is ln|1 + x| + C. So putting it all together with the coefficients:

(1/2)[ -ln|1 - x| + ln|1 + x| ] evaluated from -1/2 to 1/2. Simplifying, that's (1/2)[ ln|1 + x| - ln|1 - x| ] from -1/2 to 1/2.

Let me compute the definite integral. First, plug in the upper limit x = 1/2:

(1/2)[ ln(1 + 1/2) - ln(1 - 1/2) ] = (1/2)[ ln(3/2) - ln(1/2) ].

Similarly, plug in the lower limit x = -1/2:

(1/2)[ ln(1 + (-1/2)) - ln(1 - (-1/2)) ] = (1/2)[ ln(1/2) - ln(3/2) ].

Subtracting the lower limit result from the upper limit:

(1/2)[ (ln(3/2) - ln(1/2)) - (ln(1/2) - ln(3/2)) ].

Let me compute each part. First, ln(3/2) - ln(1/2) is ln(3/2 / (1/2)) = ln(3). Similarly, ln(1/2) - ln(3/2) is ln( (1/2)/(3/2) ) = ln(1/3) = -ln(3). So the expression becomes:

(1/2)[ ln(3) - (-ln(3)) ] = (1/2)(ln(3) + ln(3)) = (1/2)(2 ln(3)) = ln(3).

Wait, that's interesting. So the integral from -1/2 to 1/2 of 1/(1 - x²) dx is ln(3). Let me verify that again. When I substitute the upper and lower limits, the terms with ln(1/2) should cancel out properly. Let me recheck the substitution:

Upper limit x=1/2:

ln(1 + 1/2) = ln(3/2), ln(1 - 1/2) = ln(1/2). So the difference is ln(3/2) - ln(1/2) = ln(3/2 / 1/2) = ln(3).

Lower limit x=-1/2:

ln(1 + (-1/2)) = ln(1/2), ln(1 - (-1/2)) = ln(3/2). So the difference is ln(1/2) - ln(3/2) = ln(1/3) = -ln(3).

So the integral is (1/2)[ ln(3) - (-ln(3)) ] = (1/2)(2 ln(3)) = ln(3). That's correct. So the exact answer is ln(3).

Now, for the numerical approximation. The natural logarithm of 3 is approximately 1.0986122886681098... Rounded to 10 decimal places, that's 1.0986122887.

Wait, let me check with a calculator. ln(3) ≈ 1.098612289. So yes, rounding to 10 decimal places would be 1.0986122887. Hmm, but let me confirm. Let me compute ln(3) using a calculator. Let's see:

3 is e^1.098612289, so e^1.0986122886681098 ≈ 3. So the numerical value is approximately 1.0986122887 when rounded to 10 decimal places.

Therefore, the exact answer is ln(3) and the numerical approximation is approximately 1.0986122887.
</think>

{"answer": "\\ln(3)", "numerical_answer": "1.0986122887"}