<think>
Okay, let's tackle this integral step by step. The problem is to compute the definite integral from 0 to 2 of x^(1/2)(2 - x)^(1/2) cosh(1 * sqrt(x(2 - x))) dx. Hmm, that looks a bit complicated, but maybe there's a substitution that can simplify it.

First, let me write down the integral again to visualize it better:

∫₀² √x √(2 - x) cosh(√[x(2 - x)]) dx

The integrand has square roots of x and (2 - x), and the argument of the hyperbolic cosine is the square root of x(2 - x). That term inside the cosh is interesting. Let me denote t = √[x(2 - x)]. Maybe substituting t could help, but I need to check if that's feasible.

Alternatively, notice that x(2 - x) is a quadratic expression. Let's see if we can complete the square or use a trigonometric substitution. The expression x(2 - x) can be rewritten as -x² + 2x = -(x² - 2x) = -(x² - 2x + 1 - 1) = -(x - 1)^2 + 1. So, x(2 - x) = 1 - (x - 1)^2. That looks like a standard form for a trigonometric substitution. Let me try substituting x - 1 = sinθ, which would make x(2 - x) = 1 - sin²θ = cos²θ. Then, the square root becomes cosθ. Let's see where this leads.

Let’s set x = 1 + sinθ. Then, dx = cosθ dθ. But we need to adjust the limits of integration. When x = 0, 0 = 1 + sinθ ⇒ sinθ = -1 ⇒ θ = -π/2. When x = 2, 2 = 1 + sinθ ⇒ sinθ = 1 ⇒ θ = π/2. So the new limits are from -π/2 to π/2. Let's manageable.

Now, let's express the integrand in terms of θ. First, √x = √(1 + sinθ) and √(2 - x) = √(1 - sinθ). Multiplying these together gives √[(1 + sinθ)(1 - sinθ)] = √(1 - sin²θ) = √(cos²θ) = |cosθ|. Since θ is between -π/2 and π/2, cosθ is non-negative, so this simplifies to cosθ.

The argument of the hyperbolic cosine is √[x(2 - x)] = cosθ, as we saw earlier. So cosh(√[x(2 - x)]) becomes cosh(cosθ).

Putting it all together, the integral becomes:

∫_{-π/2}^{π/2} [cosθ] * cosh(cosθ) * [cosθ dθ]

Wait, let's check each part. The original integrand is √x √(2 - x) cosh(...) dx. After substitution, √x √(2 - x) becomes cosθ, and dx is cosθ dθ. So the integral becomes:

∫ cosθ * cosh(cosθ) * cosθ dθ = ∫ cos²θ cosh(cosθ) dθ from -π/2 to π/2.

Hmm, that's ∫_{-π/2}^{π/2} cos²θ cosh(cosθ) dθ. Since the integrand is even (cos²θ is even, cosh(cosθ) is even because cosh is even and cosθ is even), we can rewrite this as 2 ∫₀^{π/2} cos²θ cosh(cosθ) dθ.

But integrating this still looks challenging. Maybe there's a way to express cosh(cosθ) in a series expansion and integrate term by term? Let's recall that cosh(z) = Σ_{n=0}^∞ z^{2n}/(2n)! So, substituting z = cosθ, we have:

cosh(cosθ) = Σ_{n=0}^∞ (cosθ)^{2n}/(2n)!.

Then, the integral becomes:

2 Σ_{n=0}^∞ [1/(2n)!] ∫₀^{π/2} cos²θ * cos^{2n}θ dθ = 2 Σ_{n=0}^∞ [1/(2n)!] ∫₀^{π/2} cos^{2n + 2}θ dθ.

Now, the integral of cos^{2m}θ dθ from 0 to π/2 is known and given by the beta function or the gamma function. Specifically, ∫₀^{π/2} cos^{2m}θ dθ = (sqrt(π)/2) Γ(m + 1/2)/Γ(m + 1). Alternatively, using the formula for even powers:

∫₀^{π/2} cos^{2k}θ dθ = (π/2) * ( (2k)! ) / (4^k (k!)^2 )

But let me confirm. The standard result is ∫₀^{π/2} cos^{2k}θ dθ = (π/2) * ( (2k - 1)!! ) / (2k!! ) ) = (π/2) * ( (2k)! ) / (4^k (k!)^2 )

Yes, that's correct. So for our case, 2n + 2 = 2(n + 1), so m = n + 1. Therefore,

∫₀^{π/2} cos^{2(n + 1)}θ dθ = (π/2) * (2(n + 1))! ) / (4^{n + 1} ( (n + 1)! )^2 )

Therefore, substituting back into the series:

2 * Σ_{n=0}^∞ [1/(2n)!] * (π/2) * (2(n + 1))! / (4^{n + 1} ( (n + 1)! )^2 )

Simplify this expression:

= π Σ_{n=0}^∞ [1/(2n)!] * (2(n + 1))! / (4^{n + 1} ( (n + 1)! )^2 )

Let’s try to simplify the terms inside the summation. Let’s denote k = n + 1. Then when n = 0, k = 1; but since the original sum starts at n=0, k starts at 1. However, maybe we can adjust the index. Alternatively, let's see:

(2(n + 1))! / ( (n + 1)! )^2 ) is the central binomial coefficient for 2k choose k when k = n + 1. So, (2k)! / (k!^2) = C(2k, k). So, for k = n + 1, this term is C(2(n + 1), n + 1).

Therefore, the term becomes:

[ (2(n + 1))! / ( (n + 1)! )^2 ) ] / (4^{n + 1} ) = C(2(n + 1), n + 1) / 4^{n + 1}

But also, note that C(2k, k)/4^k is the central binomial coefficient divided by 4^k, which is known to be equal to (1/2^{2k}) * C(2k, k). But perhaps there's a generating function for this.

Alternatively, let's write the term as:

(2(n + 1))! / ( (n + 1)! )^2 4^{n + 1} ) = [ (2n + 2)! ) / ( (n + 1)! )^2 ) ] / 4^{n + 1}

But (2n + 2)! = (2n + 2)(2n + 1)(2n)! )

Similarly, (n + 1)! )^2 = (n + 1)^2 (n! )^2 )

But maybe this isn't helpful. Let's see if we can relate this to the original series.

Alternatively, let's factor out the 1/4^{n + 1} and the rest. Let me write the term as [ (2(n + 1))! / ( (n + 1)! )^2 ) ] * 1/4^{n + 1} = [ C(2(n + 1), n + 1) ] / 4^{n + 1}

But the generating function for C(2k, k)/4^k is 1/sqrt(1 - x), since Σ_{k=0}^∞ C(2k, k) x^k = 1/sqrt(1 - 4x). So, if we have x = 1/4, then Σ_{k=0}^∞ C(2k, k)/4^k x^k = 1/sqrt(1 - x). Wait, maybe not exactly. Let me check:

The generating function is Σ_{k=0}^∞ C(2k, k) x^k = 1/sqrt(1 - 4x). So, if we set x = 1/4, then Σ_{k=0}^∞ C(2k, k) (1/4)^k = 1/sqrt(1 - 1) = infinity. Hmm, that diverges. So maybe that approach isn't helpful.

Alternatively, perhaps we can manipulate the series term by term. Let's look at the ratio of consecutive terms to see if it's a hypergeometric series or something that can be summed.

But this might be getting too complicated. Let me check if there's another substitution or if the integral can be related to a known integral.

Wait, going back to the original substitution. We had x = 1 + sinθ, leading to the integral in terms of θ. But maybe there's a different substitution. Let's consider the substitution t = x - 1. Then, the integral becomes:

∫_{-1}^{1} √(1 + t) √(1 - t) cosh(√{(1 + t)(1 - t)}) dt

Which simplifies to:

∫_{-1}^1 √(1 - t²) cosh(√{1 - t²}) dt

But this is symmetric around t=0, so we can write 2 ∫₀¹ √(1 - t²) cosh(√{1 - t²}) dt

But this seems similar to the previous substitution. Maybe another substitution here. Let’s set u = √{1 - t²}. Then, u² = 1 - t², so t = √(1 - u²). Then, dt = (-u)/√(1 - u²) du. Wait, but when t goes from 0 to 1, u goes from 1 to 0. So changing the limits:

2 ∫_{u=1}^{u=0} u * cosh(u) * (-u)/√(1 - u²) du = 2 ∫₀¹ u² / √(1 - u²) cosh(u) du

Hmm, that might not be better. Alternatively, set u = t, but not sure.

Alternatively, let's consider polar coordinates or another substitution. Wait, maybe if we set v = √{1 - t²}, then v = -t / √{1 - t²} dt. Not sure.

Alternatively, perhaps integrating by parts. Let's consider the integral ∫ cos²θ cosh(cosθ) dθ. Let me see if integrating by parts would help. Let’s set u = cosθ, dv = cosθ cosh(cosθ) dθ. Hmm, not sure. Alternatively, maybe express cosh(cosθ) in terms of exponentials: cosh(z) = (e^z + e^{-z})/2. So:

cosh(cosθ) = (e^{cosθ} + e^{-cosθ})/2

So the integral becomes:

2 * ∫₀^{π/2} cos²θ * (e^{cosθ} + e^{-cosθ})/2 dθ = ∫₀^{π/2} cos²θ (e^{cosθ} + e^{-cosθ}) dθ

So, split into two integrals:

∫₀^{π/2} cos²θ e^{cosθ} dθ + ∫₀^{π/2} cos²θ e^{-cosθ} dθ

But integrating these exponentials multiplied by cos²θ might not be straightforward. Maybe expanding e^{cosθ} as a Taylor series. Let's recall that e^{cosθ} = Σ_{k=0}^∞ (cosθ)^k /k!

Similarly, e^{-cosθ} = Σ_{k=0}^∞ (-cosθ)^k /k!

So substituting these:

First integral becomes Σ_{k=0}^∞ [1/k!] ∫₀^{π/2} cos²θ (cosθ)^k dθ = Σ_{k=0}^∞ [1/k!] ∫₀^{π/2} cos^{k + 2}θ dθ

Similarly, the second integral becomes Σ_{k=0}^∞ [(-1)^k /k!] ∫₀^{π/2} cos^{k + 2}θ dθ

So combining both integrals:

Σ_{k=0}^∞ [1/k! + (-1)^k /k! ] ∫₀^{π/2} cos^{k + 2}θ dθ

But notice that [1 + (-1)^k]/k! is zero when k is odd and 2/k! when k is even. Let’s write k = 2n for even terms:

Σ_{n=0}^∞ [2/(2n)!] ∫₀^{π/2} cos^{2n + 2}θ dθ

Which is the same as the previous series we had. So we end up back at the same point. Therefore, this approach might not be helpful.

Alternatively, perhaps there's a substitution that can turn the original integral into a standard form. Let me think again about the original integral:

∫₀² √x √(2 - x) cosh(√[x(2 - x)}) dx

Let’s make a substitution u = x - 1, which centers the interval around 0. Then x = u + 1, dx = du, and the limits become from u = -1 to u = 1. The integral becomes:

∫_{-1}^1 √(u + 1) √(1 - u) cosh(√{(u + 1)(1 - u)}) du

Simplify the terms inside the roots:

(u + 1)(1 - u) = 1 - u², so √{(u + 1)(1 - u)} = √(1 - u²). Also, √(u + 1) * √(1 - u) = √{(1 + u)(1 - u)} = √(1 - u²). Therefore, the integral simplifies to:

∫_{-1}^1 √(1 - u²) cosh(√(1 - u²)) du

Which is the same as 2 ∫₀¹ √(1 - u²) cosh(√(1 - u²)) du

Now, let’s make a substitution t = √(1 - u²). Then, t = √(1 - u²) ⇒ t² = 1 - u² ⇒ u = √(1 - t²). Wait, no, solving for u gives u = √(1 - t²) but when u is in [0,1], t is in [0,1]. Wait, when u goes from 0 to 1, t goes from 1 to 0. Let's compute du in terms of dt:

From t = √(1 - u²), then dt/du = (-u)/√(1 - u²) = -u/t. Therefore, du = - (t dt)/u. But u = √(1 - t²), so du = - (t dt)/√(1 - t²). However, when u from 0 to 1 corresponds to t from 1 to 0, so changing the limits and flipping the integral:

2 ∫₀¹ √(1 - u²) cosh(√(1 - u²)) du = 2 ∫₁⁰ t cosh(t) * (- t dt)/√(1 - t²)) = 2 ∫₀¹ t² / √(1 - t²) cosh(t) dt

So the integral becomes 2 ∫₀¹ [t² / √(1 - t²)] cosh(t) dt. Hmm, this seems more complicated. Maybe another substitution here. Let’s set t = sinφ, so that √(1 - t²) = cosφ, dt = cosφ dφ. When t=0, φ=0; t=1, φ=π/2. Then the integral becomes:

2 ∫₀^{π/2} [sin²φ / cosφ] cosh(sinφ) * cosφ dφ = 2 ∫₀^{π/2} sin²φ cosh(sinφ) dφ

Which is the same as the integral we had earlier after the first substitution. So we’re going in circles.

Perhaps another approach. Let's consider the original integral and see if it's related to Bessel functions or modified Bessel functions. The presence of cosh might hint at modified Bessel functions of the first kind. Let me recall that the modified Bessel function of the first kind has an integral representation:

I_ν(z) = (1/π) ∫₀^π e^{z cosθ} cos(νθ) dθ

But our integral involves cosh(√{x(2 - x)}) which is transformed into cosh(cosθ). Maybe there's a connection here. Alternatively, perhaps using the series expansion of cosh and integrating term by term.

Let’s try that. Let's go back to the original integral after substitution:

Integral = 2 ∫₀^{π/2} cos²θ cosh(cosθ) dθ

Expand cosh(cosθ) as Σ_{n=0}^∞ (cosθ)^{2n}/(2n)!.

Then, Integral = 2 Σ_{n=0}^∞ [1/(2n)!] ∫₀^{π/2} cos^{2n + 2}θ dθ

As before, the integral of cos^{2n + 2}θ dθ from 0 to π/2 is (sqrt(π)/2) Γ(n + 3/2)/Γ(n + 2). Using the formula for the beta function:

∫₀^{π/2} cos^{2k}θ dθ = (π/2) ( (2k)! ) / (4^k (k!)^2 )

So here, k = n + 1. Therefore,

∫₀^{π/2} cos^{2n + 1}θ dθ = (π/2) ( (2(n + 1))! ) / (4^{n + 1} ( (n + 1)! )^2 )

Wait, substituting k = n + 1, so:

∫₀^{π/2} cos^{2(n + 1)}θ dθ = (π/2) ( (2(n + 1))! ) / (4^{n + 1} ( (n + 1)! )^2 )

Therefore, the integral becomes:

2 * Σ_{n=0}^∞ [1/(2n)!] * (π/2) * (2(n + 1))! / (4^{n + 1} ( (n + 1)! )^2 )

Simplify this expression:

= π Σ_{n=0}^∞ [ (2(n + 1))! / ( (2n)! (n + 1)!^2 ) ] * 1 / 4^{n + 1}

Let’s try to simplify the ratio of factorials. Let's write (2(n + 1))! = (2n + 2)! = (2n + 2)(2n + 1)(2n)! )

So,

[ (2(n + 1))! ] / [ (2n)! (n + 1)!^2 ) ] = [ (2n + 2)(2n + 1)(2n)! ) ] / [ (2n)! ( (n + 1)! )^2 ) ] = (2n + 2)(2n + 1) / ( (n + 1)! )^2 )

But (n + 1)! = (n + 1) n!, so (n + 1)!^2 = (n + 1)^2 (n! )^2 )

Therefore,

= (2n + 2)(2n + 1) / ( (n + 1)^2 (n! )^2 )

But 2n + 2 = 2(n + 1), so:

= 2(n + 1)(2n + 1) / ( (n + 1)^2 (n! )^2 ) = 2(2n + 1) / ( (n + 1) (n! )^2 )

Therefore, the term inside the summation becomes:

2(2n + 1) / ( (n + 1) (n! )^2 ) * 1 / 4^{n + 1} = 2(2n + 1) / ( (n + 1) (n! )^2 4^{n + 1} )

Simplify the constants:

2 / 4^{n + 1} = 2 / (4 * 4^n) = 1/(2 * 4^n )

So,

= (2n + 1) / ( (n + 1) (n! )^2 2 * 4^n )

= (2n + 1) / ( 2 * 4^n (n + 1) (n! )^2 )

Hmm, this seems complicated, but maybe we can relate this to known series. Let's see:

Let’s write the term as:

(2n + 1) / (2 * 4^n (n + 1) (n! )^2 ) = (2n + 1) / (2 * 4^n (n + 1) (n! )^2 )

Let’s split the numerator:

= [ (2n + 1) / (n + 1) ] * 1/(2 * 4^n (n! )^2 )

But (2n + 1)/(n + 1) = 2 - 1/(n + 1). Not sure if that helps.

Alternatively, perhaps express 2n + 1 as (n + 1) + n. So:

= [ (n + 1) + n ] / (n + 1) * 1/(2 * 4^n (n! )^2 )

= [1 + n/(n + 1)] * 1/(2 * 4^n (n! )^2 )

Still not helpful. Maybe we can find a generating function for this series. Let's see:

The term is (2n + 1)/(2 * 4^n (n + 1) (n! )^2 )

Let’s consider changing the index. Let m = n + 1. Then n = m - 1. When n = 0, m = 1. So:

Σ_{n=0}^∞ [ (2n + 1) / (2 * 4^n (n + 1) (n! )^2 ) ] = Σ_{m=1}^∞ [ (2(m - 1) + 1) / (2 * 4^{m - 1} m ( (m - 1)! )^2 ) ]

= Σ_{m=1}^∞ [ (2m - 1) / (2 * 4^{m - 1} m ( (m - 1)! )^2 ) ]

But this:

= Σ_{m=1}^∞ [ (2m - 1) / (2 * 4^{m - 1} m ( (m - 1)! )^2 ) ]

= Σ_{m=1}^∞ [ (2m - 1) * 4 / (2 * 4^m m ( (m - 1)! )^2 ) ]

= Σ_{m=1}^∞ [ (2m - 1) * 2 / (4^m m ( (m - 1)! )^2 ) ]

Hmm, not sure. Alternatively, perhaps this series can be expressed in terms of known functions. Let me think about known series involving factorial terms.

Alternatively, perhaps the original integral can be expressed in terms of Bessel functions. Let me recall that integrals involving cosh(a cosθ) can be related to modified Bessel functions. For example, the modified Bessel function of the first kind has an integral representation:

I_ν(z) = (1/π) ∫₀^π e^{z cosθ} cos(νθ) dθ

But we have cosh(cosθ) which is (e^{cosθ} + e^{-cosθ})/2. So, integrating cosh(cosθ) times cos²θ might relate to I_0(1) or similar.

Wait, let's consider the integral ∫₀^{π/2} cos²θ cosh(cosθ) dθ. Let's write cos²θ = (1 + cos2θ)/2. Then:

∫₀^{π/2} (1 + cos2θ)/2 cosh(cosθ) dθ = (1/2) ∫₀^{π/2} cosh(cosθ) dθ + (1/2) ∫₀^{π/2} cos2θ cosh(cosθ) dθ

But I'm not sure if this helps. Let's compute each integral separately.

First integral: (1/2) ∫₀^{π/2} cosh(cosθ) dθ

Second integral: (1/2) ∫₀^{π/2} cos2θ cosh(cosθ) dθ

The first integral is related to the modified Bessel function. Specifically, I_0(1) = (1/π) ∫₀^π e^{cosθ} dθ. Similarly, integrating cosh(cosθ) over 0 to π/2 would relate to I_0(1) but scaled.

But let's compute ∫₀^{π/2} cosh(cosθ) dθ. Since cosh(cosθ) = (e^{cosθ} + e^{-cosθ})/2, so:

∫₀^{π/2} cosh(cosθ) dθ = (1/2) [ ∫₀^{π/2} e^{cosθ} dθ + ∫₀^{π/2} e^{-cosθ} dθ ]

But these integrals don't have elementary forms, but they can be expressed in terms of Bessel functions. Specifically, ∫₀^π e^{a cosθ} dθ = π I_0(a). So, ∫₀^{π/2} e^{cosθ} dθ is half of that integral from 0 to π, but not exactly. Wait, no. The integral from 0 to π/2 is not directly related. However, we can express it in terms of the modified Bessel function.

But perhaps there's a relation. Let me recall that:

I_ν(z) = (1/π) ∫₀^π e^{z cosθ} cos(νθ) dθ

For ν = 0, I_0(z) = (1/π) ∫₀^π e^{z cosθ} dθ. Therefore, ∫₀^π e^{z cosθ} dθ = π I_0(z). Similarly, ∫₀^{π/2} e^{z cosθ} dθ = (π/2) I_0(z) + ...? Not sure. Maybe not directly.

Alternatively, we can use the series expansion of e^{cosθ} and integrate term by term. Let's try that.

e^{cosθ} = Σ_{k=0}^∞ (cosθ)^k /k!

Therefore, ∫₀^{π/2} e^{cosθ} dθ = Σ_{k=0}^∞ [1/k!] ∫₀^{π/2} cos^kθ dθ

Similarly, the integral of cos^kθ from 0 to π/2 is (sqrt(π)/2) Γ((k + 1)/2)/Γ((k + 2)/2)

But this might not help in summing the series. However, for even and odd k:

For even k = 2m: ∫₀^{π/2} cos^{2m}θ dθ = (π/2) (2m)! / (4^m (m! )^2 )

For odd k = 2m + 1: ∫₀^{π/2} cos^{2m + 1}θ dθ = (2^m m! ) / ( (2m + 1)!! )

But this complicates the series. However, perhaps we can write:

∫₀^{π/2} e^{cosθ} dθ = Σ_{m=0}^∞ [1/(2m)!] ∫₀^{π/2} cos^{2m}θ dθ + Σ_{m=0}^∞ [1/(2m + 1)!] ∫₀^{π/2} cos^{2m + 1}θ dθ

But this seems messy. Maybe it's better to accept that this integral can't be expressed in closed form and look for another approach.

Wait, going back to the original problem. The integral is from 0 to 2 of √x √(2 - x) cosh(√{x(2 - x)}) dx. Let's consider another substitution. Let’s set y = x(2 - x). Then, dy/dx = 2 - 2x. But this might not be helpful. Alternatively, set t = √{x(2 - x)}. Then, t² = x(2 - x). Differentiating both sides: 2t dt/dx = 2 - 2x. So, dt/dx = (1 - x)/t. But this seems to complicate things.

Alternatively, let's consider parametrizing x as x = 2 sin²(θ/2). Then, 2 - x = 2 cos²(θ/2). Then, x(2 - x) = 4 sin²(θ/2) cos²(θ/2) = sin²θ. So √{x(2 - x)} = sinθ. Then, dx = 2 sin(θ/2) cos(θ/2) dθ = sinθ dθ. The limits: when x=0, θ=0; when x=2, θ=π. So the integral becomes:

∫₀^π √{2 sin²(θ/2)} √{2 cos²(θ/2)} cosh(sinθ) * sinθ dθ

Simplify the square roots:

√{2 sin²(θ/2)} = √2 sin(θ/2)

√{2 cos²(θ/2)} = √2 cos(θ/2)

Multiplying these gives √2 sin(θ/2) * √2 cos(θ/2) = 2 sin(θ/2) cos(θ/2) = sinθ

So the integral becomes:

∫₀^π sinθ * cosh(sinθ) * sinθ dθ = ∫₀^π sin²θ cosh(sinθ) dθ

Hmm, this seems similar to the previous integrals we had. But integrating sin²θ cosh(sinθ) from 0 to π. This might not be easier, but perhaps expanding cosh(sinθ) in a series.

cosh(sinθ) = Σ_{n=0}^∞ (sinθ)^{2n}/(2n)!.

Thus, the integral becomes:

Σ_{n=0}^∞ [1/(2n)!] ∫₀^π sin^{2n + 2}θ dθ

But the integral of sin^{2k}θ from 0 to π is 2 ∫₀^{π/2} sin^{2k}θ dθ = 2 * (π/2) ( (2k)! ) / (4^k (k! )^2 ) = π (2k)! / (4^k (k! )^2 )

Therefore, the integral becomes:

Σ_{n=0}^∞ [1/(2n)!] * π (2(n + 1))! / (4^{n + 1} ( (n + 1)! )^2 )

Which is the same series as before. So again, we end up with the same expression.

This suggests that the integral might not have a closed-form solution in terms of elementary functions and might need to be expressed as a series or in terms of special functions. However, the problem states to compute the integral analytically to obtain the exact answer. This implies that there might be a clever substitution or identity that I'm missing.

Let me think differently. The original integral is:

∫₀² √x √(2 - x) cosh(√{x(2 - x)}) dx

Let’s consider the substitution t = x - 1, which we did earlier, leading to:

2 ∫₀¹ √(1 - t²) cosh(√{1 - t²}) dt

Let’s make a substitution u = √{1 - t²}, so t = √{1 - u²}, dt = -u / √{1 - u²} du. Wait, when t goes from 0 to 1, u goes from 1 to 0. So:

2 ∫₁⁰ √(1 - t²) cosh(u) * (-u / √{1 - u²}) du = 2 ∫₀¹ u * cosh(u) * (u / √{1 - u²}) du

= 2 ∫₀¹ u² / √{1 - u²} cosh(u) du

Hmm, this seems similar to what we had before. Let’s try integrating by parts here. Let’s set:

Let’s set v = u sinh(u), dv = sinh(u) + u cosh(u) du

Wait, maybe not. Let’s set:

Let’s set w = u, dv = u / √{1 - u²} cosh(u) du

But this might not help. Alternatively, let’s set:

Let’s set v = sinh(u), but not sure.

Alternatively, consider expanding cosh(u) into its Taylor series:

cosh(u) = Σ_{n=0}^∞ u^{2n}/(2n)!

Then, the integral becomes:

2 Σ_{n=0}^∞ [1/(2n)!] ∫₀¹ u^{2n + 2} / √{1 - u²} du

The integral ∫₀¹ u^{2n + 2} / √{1 - u²} du can be expressed in terms of the beta function. Let’s make a substitution s = u², so ds = 2u du, but not sure. Alternatively, set s = u², then u = sqrt(s), du = (1/(2 sqrt(s))) ds. Then:

∫₀¹ u^{2n + 2} / √{1 - u²} du = ∫₀¹ s^{n + 1} / √{1 - s} * (1/(2 sqrt(s))) ds = (1/2) ∫₀¹ s^{n + 1/2} (1 - s)^{-1/2} ds

This is (1/2) B(n + 3/2, 1/2) where B is the beta function. The beta function B(a, b) = Γ(a)Γ(b)/Γ(a + b). So:

(1/2) Γ(n + 3/2)Γ(1/2)/Γ(n + 2)

We know that Γ(1/2) = sqrt(π), and Γ(n + 3/2) = (n + 1/2) Γ(n + 1/2). Also, Γ(n + 2) = (n + 1)!.

Using the property of the gamma function, Γ(n + 1/2) = (2n)! sqrt(π) / 4^n n! )

Wait, Γ(n + 1/2) = (2n)! / (4^n n! ) sqrt(π). So:

Γ(n + 3/2) = (n + 1/2) Γ(n + 1/2) = (n + 1/2) * (2n)! / (4^n n! ) sqrt(π)

Therefore,

B(n + 3/2, 1/2) = Γ(n + 3/2)Γ(1/2)/Γ(n + 2) = [ (n + 1/2) (2n)! sqrt(π) / 4^n n! ) ] * sqrt(π) / (n + 1)! )

Simplify:

= (n + 1/2) (2n)! π / (4^n n! (n + 1)! ) )

But (n + 1/2) = (2n + 1)/2, so:

= (2n + 1)/2 * (2n)! π / (4^n n! (n + 1)! ) )

Therefore, the integral ∫₀¹ u^{2n + 2} / √{1 - u²} du = (1/2) B(n + 3/2, 1/2) = (1/2) * (2n + 1)/2 * (2n)! π / (4^n n! (n + 1)! ) )

= (2n + 1) (2n)! π / (4^{n + 1} n! (n + 1)! ) )

Therefore, the original series becomes:

2 Σ_{n=0}^∞ [1/(2n)!] * (2n + 1) (2n)! π / (4^{n + 1} n! (n + 1)! ) )

Simplify:

= 2 π Σ_{n=0}^∞ [ (2n + 1) / (4^{n + 1} n! (n + 1)! ) ]

= (2 π / 4) Σ_{n=0}^∞ [ (2n + 1) / (4^n n! (n + 1)! ) ]

= (π / 2) Σ_{n=0}^∞ (2n + 1) / (4^n n! (n + 1)! )

Now, let's see if this series can be summed. Let’s write the term as:

(2n + 1)/(4^n n! (n + 1)! ) = [2n + 1]/[4^n n! (n + 1)! ]

Let’s split the numerator:

= [2(n + 1) - 1]/[4^n n! (n + 1)! ]

= 2(n + 1)/[4^n n! (n + 1)! ] - 1/[4^n n! (n + 1)! ]

= 2/[4^n n! (n)! ] - 1/[4^n n! (n + 1)! ]

= 2/(4^n (n! )^2 ) - 1/(4^n n! (n + 1)! )

Therefore, the series becomes:

Σ_{n=0}^∞ [2/(4^n (n! )^2 ) - 1/(4^n n! (n + 1)! ) ] = 2 Σ_{n=0}^∞ 1/(4^n (n! )^2 ) - Σ_{n=0}^∞ 1/(4^n n! (n + 1)! )

Let’s compute each series separately.

First series: S1 = 2 Σ_{n=0}^∞ 1/(4^n (n! )^2 )

This is 2 times the sum of (1/4)^n / (n! )^2. Recall that the modified Bessel function of the first kind I_0(z) = Σ_{n=0}^∞ (z^{2n} ) / (4^n (n! )^2 ). So, if we set z = 1, then I_0(1) = Σ_{n=0}^∞ 1/(4^n (n! )^2 ). Therefore, S1 = 2 I_0(1)

Second series: S2 = Σ_{n=0}^∞ 1/(4^n n! (n + 1)! )

Let’s adjust the index. Let m = n + 1. Then when n=0, m=1:

S2 = Σ_{m=1}^∞ 1/(4^{m - 1} (m - 1)! m! ) = 4 Σ_{m=1}^∞ 1/(4^m (m - 1)! m! )

But this can be written as 4 Σ_{m=1}^∞ 1/(4^m (m - 1)! m! ) = 4 Σ_{k=0}^∞ 1/(4^{k + 1} k! (k + 1)! ) ) where k = m - 1.

= (4/4) Σ_{k=0}^∞ 1/(4^k k! (k + 1)! ) ) = Σ_{k=0}^∞ 1/(4^k k! (k + 1)! )

But this is similar to the series for I_1(1), the modified Bessel function of the first kind of order 1. Recall that I_1(z) = Σ_{k=0}^∞ (z^{2})^{2k + 1} / (k! (k + 1)! )

Wait, let's check:

I_ν(z) = Σ_{k=0}^∞ (z/2)^{2k + ν} / (k! Γ(k + ν + 1))

For ν=1, I_1(z) = Σ_{k=0}^∞ (z/2)^{2k + 1} / (k! (k + 1)! )

So, for z=2, I_1(2) = Σ_{k=0}^∞ (1)^{2k + 1} / (k! (k + 1)! ) = Σ_{k=0}^∞ 1/(k! (k + 1)! )

But our series S2 = Σ_{k=0}^∞ 1/(4^k k! (k + 1)! )

This is similar but with an additional factor of 1/4^k. So, perhaps we can relate this to I_1(1). Let’s see:

If we set z=1, then I_1(1) = Σ_{k=0}^∞ (1/2)^{2k + 1} / (k! (k + 1)! ) = Σ_{k=0}^∞ 1/(2^{2k + 1} k! (k + 1)! ) = (1/2) Σ_{k=0}^∞ 1/(4^k k! (k + 1)! )

Therefore, Σ_{k=0}^∞ 1/(4^k k! (k + 1)! ) = 2 I_1(1)

Therefore, S2 = 2 I_1(1)

Putting it all together:

Integral = (π/2)(S1 - S2) = (π/2)(2 I_0(1) - 2 I_1(1)) = π (I_0(1) - I_1(1))

So the exact answer is π (I_0(1) - I_1(1)), where I_0 and I_1 are modified Bessel functions of the first kind.

Now, we need to compute the numerical approximation. Let's recall the values of I_0(1) and I_1(1).

The modified Bessel function I_0(1) can be calculated as:

I_0(1) ≈ 1.2660658787528354

I_1(1) ≈ 0.565159103992485

Therefore, I_0(1) - I_1(1) ≈ 1.2660658787528354 - 0.565159103992485 ≈ 0.7009067747603504

Then, multiplying by π:

π * 0.7009067747603504 ≈ 2.202158889089356

Rounded to 10 decimal places, this is approximately 2.2021588891.

Therefore, the exact answer is π (I₀(1) − I₁(1)) and the numerical approximation is approximately 2.2021588891.
</think>

{"answer": "\\pi \\left(I_0(1) - I_1(1)\\right)", "numerical_answer": "2.2021588891"}