# Calculating $\int_{-1}^{0}5\left(x^{6}+x\right)^{4}\:\mathrm{d}x$

## Step 1: Substitute $u = x^6 + x$
Let's set $u = x^6 + x$, then we need to find $du$:
$du = (6x^5 + 1)dx$

## Step 2: Rewrite the integral
We can't directly substitute because we need to express $dx$ in terms of $du$, and the relation is not straightforward to invert. Instead, let's try a different approach.

## Alternative approach: Substitute $x = -t$
Let's substitute $x = -t$, which means $dx = -dt$ and when $x = -1$, $t = 1$ and when $x = 0$, $t = 0$.

The integral becomes:
$$\int_{-1}^{0}5\left(x^{6}+x\right)^{4}\:\mathrm{d}x = \int_{1}^{0}5\left((-t)^{6}+(-t)\right)^{4}\:(-\mathrm{d}t)$$
$$= \int_{0}^{1}5\left(t^{6}-t\right)^{4}\:\mathrm{d}t$$

## Step 3: Notice the symmetry property
We need to evaluate:
$$\int_{0}^{1}5\left(t^{6}-t\right)^{4}\:\mathrm{d}t$$

Notice that when we substitute $x = -t$ in the original function, we get:
$$((-t)^6 + (-t))^4 = (t^6 - t)^4$$

This means that $f(-t) = f(t)$ where $f(t) = (t^6 + t)^4$.

Due to this symmetry property of an even function:
$$\int_{-1}^{0}5\left(x^{6}+x\right)^{4}\:\mathrm{d}x = \int_{0}^{1}5\left(x^{6}+x\right)^{4}\:\mathrm{d}x$$

## Step 4: Let's compute $\int_{0}^{1}5\left(x^{6}+x\right)^{4}\:\mathrm{d}x$
Let's set $u = x^6 + x$, then $du = (6x^5 + 1)dx$

When $x = 0$: $u = 0$
When $x = 1$: $u = 1 + 1 = 2$

We can't directly isolate $dx$, so we'll need a different substitution.

## Step 5: Use the binomial theorem
Let's expand $(x^6 + x)^4$ using the binomial theorem:

$$(x^6 + x)^4 = \sum_{k=0}^{4} \binom{4}{k} (x^6)^k (x)^{4-k} = \sum_{k=0}^{4} \binom{4}{k} x^{6k} x^{4-k} = \sum_{k=0}^{4} \binom{4}{k} x^{6k+4-k} = \sum_{k=0}^{4} \binom{4}{k} x^{5k+4}$$

So we have:
$$\int_{-1}^{0}5\left(x^{6}+x\right)^{4}\:\mathrm{d}x = 5\int_{-1}^{0}\sum_{k=0}^{4} \binom{4}{k} x^{5k+4}\:\mathrm{d}x$$

$$= 5\sum_{k=0}^{4} \binom{4}{k}\int_{-1}^{0} x^{5k+4}\:\mathrm{d}x$$

## Step 6: Compute each integral
For each value of $k$, we compute:
$$\int_{-1}^{0} x^{5k+4}\:\mathrm{d}x = \left[\frac{x^{5k+5}}{5k+5}\right]_{-1}^{0} = \frac{0^{5k+5}}{5k+5} - \frac{(-1)^{5k+5}}{5k+5} = -\frac{(-1)^{5k+5}}{5k+5}$$

For $k = 0$: $\int_{-1}^{0} x^{4}\:\mathrm{d}x = -\frac{(-1)^{5}}{5} = -\frac{-1}{5} = \frac{1}{5}$

For $k = 1$: $\int_{-1}^{0} x^{9}\:\mathrm{d}x = -\frac{(-1)^{10}}{10} = -\frac{1}{10}$

For $k = 2$: $\int_{-1}^{0} x^{14}\:\mathrm{d}x = -\frac{(-1)^{15}}{15} = -\frac{-1}{15} = \frac{1}{15}$

For $k = 3$: $\int_{-1}^{0} x^{19}\:\mathrm{d}x = -\frac{(-1)^{20}}{20} = -\frac{1}{20}$

For $k = 4$: $\int_{-1}^{0} x^{24}\:\mathrm{d}x = -\frac{(-1)^{25}}{25} = -\frac{-1}{25} = \frac{1}{25}$

## Step 7: Calculate the final result
$$5\sum_{k=0}^{4} \binom{4}{k}\int_{-1}^{0} x^{5k+4}\:\mathrm{d}x$$

$$= 5\left(\binom{4}{0}\frac{1}{5} + \binom{4}{1}\left(-\frac{1}{10}\right) + \binom{4}{2}\frac{1}{15} + \binom{4}{3}\left(-\frac{1}{20}\right) + \binom{4}{4}\frac{1}{25}\right)$$

$$= 5\left(1 \cdot \frac{1}{5} + 4 \cdot \left(-\frac{1}{10}\right) + 6 \cdot \frac{1}{15} + 4 \cdot \left(-\frac{1}{20}\right) + 1 \cdot \frac{1}{25}\right)$$

$$= 5\left(\frac{1}{5} - \frac{4}{10} + \frac{6}{15} - \frac{4}{20} + \frac{1}{25}\right)$$

$$= 5\left(\frac{5}{25} - \frac{10}{25} + \frac{10}{25} - \frac{5}{25} + \frac{1}{25}\right)$$

$$= 5 \cdot \frac{1}{25} = \frac{5}{25} = \frac{1}{5}$$

Therefore, $\int_{-1}^{0}5\left(x^{6}+x\right)^{4}\:\mathrm{d}x = \frac{1}{5}$

## Step 8: Numerical approximation
$\frac{1}{5} = 0.2$ exactly.

{"answer": "\\frac{1}{5}", "numerical_answer": "0.2000000000"}