

To solve the definite integral \(\int\limits_0^2 x^{-1/2} H_{3}\left(\sqrt[4]{x(2-x)}\right) dx\), we follow these steps:

### Step 1: Expand the Hermite polynomial
The 3rd Hermite polynomial is \(H_3(z) = 8z^3 - 12z\). Substituting \(z = \sqrt[4]{x(2-x)}\), we get:
\[
H_3\left(\sqrt[4]{x(2-x)}\right) = 8\left(x(2-x)\right)^{3/4} - 12\left(x(2-x)\right)^{1/4}.
\]

### Step 2: Simplify the integrand
The integrand becomes:
\[
x^{-1/2} \left[8\left(x(2-x)\right)^{3/4} - 12\left(x(2-x)\right)^{1/4}\right].
\]
Simplifying each term:
- First term: \(8x^{-1/2} \cdot x^{3/4}(2-x)^{3/4} = 8x^{1/4}(2-x)^{3/4}\),
- Second term: \(-12x^{-1/2} \cdot x^{1/4}(2-x)^{1/4} = -12x^{-1/4}(2-x)^{1/4}\).

Thus, the integral splits into two parts:
\[
\int_0^2 x^{-1/2} H_3\left(\sqrt[4]{x(2-x)}\right) dx = 8 \int_0^2 x^{1/4}(2-x)^{3/4} dx - 12 \int_0^2 x^{-1/4}(2-x)^{1/4} dx.
\]

### Step 3: Evaluate the integrals using the Beta function
The integrals are of the form \(\int_0^a t^{p-1}(a-t)^{q-1} dt\), which relates to the Beta function \(B(p, q) = \int_0^1 t^{p-1}(1-t)^{q-1} dt\) via substitution \(t = au\). For \(a = 2\):

1. **First integral**: \(\int_0^2 x^{1/4}(2-x)^{3/4} dx\)
   - Substitute \(x = 2u\), \(dx = 2du\). The integral becomes:
     \[
     2^{1/4 + 3/4 + 1} \int_0^1 u^{1/4}(1-u)^{3/4} du = 4 \cdot B\left(\frac{5}{4}, \frac{7}{4}\right).
     \]
   - Using \(B(p, q) = \frac{\Gamma(p)\Gamma(q)}{\Gamma(p+q)}\), and \(\Gamma(3) = 2!\), we find:
     \[
     B\left(\frac{5}{4}, \frac{7}{4}\right) = \frac{\Gamma\left(\frac{5}{4}\right)\Gamma\left(\frac{7}{4}\right)}{\Gamma(3)} = \frac{\left(\frac{1}{4}\Gamma\left(\frac{1}{4}\right)\right)\left(\frac{3}{4}\Gamma\left(\frac{3}{4}\right)\right)}{2} = \frac{3\pi\sqrt{2}}{32}.
     \]
   - Thus, the first integral is \(4 \cdot \frac{3\pi\sqrt{2}}{32} = \frac{3\pi\sqrt{2}}{8}\).

2. **Second integral**: \(\int_0^2 x^{-1/4}(2-x)^{1/4} dx\)
   - Substitute \(x = 2u\), \(dx = 2du\). The integral becomes:
     \[
     2 \cdot B\left(\frac{3}{4}, \frac{5}{4}\right).
     \]
   - Using \(B\left(\frac{3}{4}, \frac{5}{4}\right) = \frac{\Gamma\left(\frac{3}{4}\right)\Gamma\left(\frac{5}{4}\right)}{\Gamma(2)} = \frac{\pi\sqrt{2}}{4}\), the second integral is \(2 \cdot \frac{\pi\sqrt{2}}{4} = \frac{\pi\sqrt{2}}{2}\).

### Step 4: Combine the results
The original integral is:
\[
8 \cdot \frac{3\pi\sqrt{2}}{8} - 12 \cdot \frac{\pi\sqrt{2}}{2} = 3\pi\sqrt{2} - 6\pi\sqrt{2} = -3\pi\sqrt{2}.
\]

### Step 5: Numerical approximation
Using \(\pi \approx 3.141592653589793\) and \(\sqrt{2} \approx 1.4142135623730951\), we get:
\[
-3\pi\sqrt{2} \approx -13.3286487257.
\]

{"answer": "-3\\pi\\sqrt{2}", "numerical_answer": "-13.3286487257"}