Let’s calculate the integral:

\[
I = \int_0^1 x \arcsin x \arccos x \, dx
\]

**Step 1: Analytical Calculation**

Recall that \(\arcsin x + \arccos x = \frac{\pi}{2}\):

So \(\arccos x = \frac{\pi}{2} - \arcsin x\). Substitute into the integral:

\[
I = \int_0^1 x \arcsin x \left(\frac{\pi}{2} - \arcsin x\right) dx
= \frac{\pi}{2} \int_0^1 x \arcsin x \, dx - \int_0^1 x (\arcsin x)^2 dx
\]

Define:
- \(A := \int_0^1 x \arcsin x \, dx\)
- \(B := \int_0^1 x (\arcsin x)^2 dx\)

So:

\[
I = \frac{\pi}{2} A - B
\]

We will now compute \(A\) and \(B\).

---

**Compute \(A = \int_0^1 x \arcsin x \, dx\):**

Let’s use integration by parts:

Let \(u = \arcsin x\), \(dv = x \, dx\). Then \(du = \frac{1}{\sqrt{1-x^2}}dx\), \(v = \frac{1}{2}x^2\).

So:

\[
A = \left. \arcsin x \cdot \frac{1}{2}x^2 \right|_{x=0}^{x=1} - \int_0^1 \frac{1}{2}x^2 \cdot \frac{1}{\sqrt{1-x^2}}dx 
\]

Evaluate the boundary term:
- At \(x=1\): \(\arcsin 1 = \frac{\pi}{2}\), so \(\frac{1}{2}x^2 = \frac{1}{2}\).
- At \(x=0\): \(\arcsin 0 = 0\), so the term is 0.

So
\[
\left. \arcsin x \cdot \frac{1}{2}x^2 \right|_0^1 = \frac{\pi}{4}
\]

Now, tackle the remaining integral:
\[
I_1 := \int_0^1 \frac{x^2}{\sqrt{1-x^2}} dx
\]

Let \(x = \sin \theta\), \(dx = \cos \theta d\theta\), \(x^2 = \sin^2\theta\), \(\sqrt{1-x^2} = \cos \theta\). As \(x\) varies from 0 to 1, \(\theta\) varies from 0 to \(\frac{\pi}{2}\).

\[
I_1 = \int_{\theta=0}^{\theta=\frac{\pi}{2}} \frac{\sin^2\theta}{\cos\theta} \cos\theta d\theta = \int_0^{\frac{\pi}{2}} \sin^2\theta d\theta
\]

But \(\int \sin^2 \theta d\theta = \int \frac{1 - \cos 2\theta}{2} d\theta = \frac{\theta}{2} - \frac{\sin 2\theta}{4} + C\).

Evaluate from 0 to \(\frac{\pi}{2}\):

\[
I_1 = \left[ \frac{\theta}{2} - \frac{\sin 2\theta}{4} \right]_0^{\frac{\pi}{2}}
 = \left( \frac{\pi}{4} - \frac{0}{4} \right) - \left( 0 - 0 \right) = \frac{\pi}{4}
\]

So the full result for \(A\):

\[
A = \frac{\pi}{4} - \frac{1}{2} \left(\frac{\pi}{4}\right) = \frac{\pi}{4} - \frac{\pi}{8} = \frac{\pi}{8}
\]

---

**Compute \(B = \int_0^1 x (\arcsin x)^2 dx\):**

Integration by parts:

Let \(u = (\arcsin x)^2\), \(dv = x dx\); then \(du = 2 \arcsin x \cdot \frac{1}{\sqrt{1-x^2}}dx\), \(v = \frac{1}{2}x^2\).

So:

\[
B = \left. (\arcsin x)^2 \cdot \frac{1}{2} x^2 \right|_0^1 - \int_0^1 \frac{1}{2} x^2 \cdot 2 \arcsin x \cdot \frac{1}{\sqrt{1-x^2}} dx
\]
\[
= \left. \frac{1}{2} x^2 (\arcsin x)^2 \right|_0^1 - \int_0^1 x^2 \arcsin x \cdot \frac{1}{\sqrt{1-x^2}} dx
\]

Evaluate the boundary term:
- At \(x=1\): \(x^2 = 1\), \(\arcsin 1 = \frac{\pi}{2}\): So \(\frac{1}{2} (\frac{\pi}{2})^2 = \frac{\pi^2}{8}\).
- At \(x=0\): zero.

So the boundary term is \(\frac{\pi^2}{8}\).

Let’s denote:
\[
I_2 := \int_0^1 x^2 \arcsin x \cdot \frac{1}{\sqrt{1-x^2}} dx
\]

Again, use the substitution \(x = \sin\theta\):

- \(dx = \cos\theta d\theta\)
- \(x^2 = \sin^2\theta\)
- \(\arcsin x = \theta\)
- \(\sqrt{1 - x^2} = \cos\theta\)

So:
\[
I_2 = \int_{x=0}^{x=1} x^2 \arcsin x \frac{1}{\sqrt{1-x^2}} dx
 = \int_{\theta=0}^{\theta=\frac{\pi}{2}} \sin^2\theta \cdot \theta \frac{1}{\cos\theta} \cos\theta d\theta
 = \int_0^{\frac{\pi}{2}} \sin^2\theta \cdot \theta d\theta
\]

So:

\[
B = \frac{\pi^2}{8} - \int_0^{\frac{\pi}{2}} \theta \sin^2\theta d\theta
\]

---

**Thus, the original integral is:**

\[
I = \frac{\pi}{2}A - B = \frac{\pi}{2} \left(\frac{\pi}{8}\right) - \left[ \frac{\pi^2}{8} - \int_0^{\frac{\pi}{2}} \theta \sin^2\theta d\theta \right]
\]
\[
= \frac{\pi^2}{16} - \frac{\pi^2}{8} + \int_0^{\frac{\pi}{2}} \theta \sin^2\theta d\theta
\]
\[
= -\frac{\pi^2}{16} + \int_0^{\frac{\pi}{2}} \theta \sin^2\theta d\theta
\]

Let’s compute the remaining integral:

\[
J = \int_0^{\frac{\pi}{2}} \theta \sin^2\theta d\theta
\]

Recall: \(\sin^2\theta = \frac{1}{2}(1 - \cos 2\theta)\):

\[
J = \int_0^{\frac{\pi}{2}} \theta \frac{1}{2}(1 - \cos 2\theta) d\theta
= \frac{1}{2} \int_0^{\frac{\pi}{2}} \theta d\theta - \frac{1}{2} \int_0^{\frac{\pi}{2}} \theta \cos 2\theta d\theta
\]

Compute each term:

1. \(\int_0^{\frac{\pi}{2}} \theta d\theta = \left. \frac{\theta^2}{2} \right|_0^{\frac{\pi}{2}} = \frac{1}{2} \left( \frac{\pi^2}{4} \right) = \frac{\pi^2}{8}\)

2. Compute \(\int_0^{\frac{\pi}{2}} \theta \cos 2\theta d\theta\):

Let’s use integration by parts:

Let \(u = \theta\), \(dv = \cos 2\theta d\theta\), so \(du = d\theta\), \(v = \frac{1}{2} \sin 2\theta\).

\[
\int \theta \cos 2\theta d\theta = \theta \cdot \frac{1}{2} \sin 2\theta - \int \frac{1}{2} \sin 2\theta d\theta
= \frac{\theta}{2} \sin 2\theta + \frac{1}{4} \cos 2\theta + C
\]

Evaluate from 0 to \(\frac{\pi}{2}\):

First, \(\sin 2\theta\) at \(\theta = \frac{\pi}{2}\) is \(\sin \pi = 0\), at \(\theta = 0\), is 0.

\(\cos 2\theta\) at \(\theta = \frac{\pi}{2}\) is \(\cos \pi = -1\), at 0 it's 1.

So, the definite integral:

\[
\int_0^{\frac{\pi}{2}} \theta \cos 2\theta d\theta = 
\left[ \frac{\theta}{2} \sin 2\theta + \frac{1}{4} \cos 2\theta \right]_0^{\frac{\pi}{2}}
= \left( \frac{\frac{\pi}{2}}{2} \cdot 0 + \frac{1}{4}(-1) \right) - \left( 0 + \frac{1}{4}(1) \right)
= \left( 0 - \frac{1}{4} \right) - \left( 0 + \frac{1}{4} \right)
= -\frac{1}{4} - \frac{1}{4} = -\frac{1}{2}
\]

Therefore,

\[
J = \frac{1}{2} \cdot \frac{\pi^2}{8} - \frac{1}{2} \cdot \left(-\frac{1}{2}\right) = \frac{\pi^2}{16} + \frac{1}{4}
\]

---

**Plug back into the result for \(I\):**

\[
I = -\frac{\pi^2}{16} + \left( \frac{\pi^2}{16} + \frac{1}{4} \right ) = \frac{1}{4}
\]

---

**Step 2: Final Exact Answer**

\[
\boxed{\int\limits_0^1 x \arcsin x \arccos x dx = \frac{1}{4}}
\]

---

**Step 3: Numerical Approximation**

\[
\frac{1}{4} = 0.25
\]
To 10 decimal places, that's:
\[
0.2500000000
\]

---

**Step 4: JSON Output**

```json
{"answer": "\\frac{1}{4}", "numerical_answer": "0.2500000000"}
```