# Evaluation of $\int_{-1}^1\frac{\cos x}{1+e^{-\frac{1}{x}}}\mathrm{d}x$

## Step 1: Analyze the integrand
Let's examine the integrand $f(x) = \frac{\cos x}{1+e^{-\frac{1}{x}}}$. 

For $x \neq 0$, we can simplify the denominator:
$1+e^{-\frac{1}{x}} = 1+\frac{1}{e^{\frac{1}{x}}} = \frac{e^{\frac{1}{x}}+1}{e^{\frac{1}{x}}} = \frac{e^{\frac{1}{x}}+1}{e^{\frac{1}{x}}}$

## Step 2: Recognize the symmetry
Let's consider the behavior of $f(-x)$:
$f(-x) = \frac{\cos(-x)}{1+e^{-\frac{1}{-x}}} = \frac{\cos x}{1+e^{\frac{1}{x}}}$

Since we're integrating over $[-1,1]$, which is symmetric about the origin, we can exploit any symmetry properties.

## Step 3: Make a substitution
For $x < 0$, $e^{-\frac{1}{x}} = e^{\frac{1}{|x|}}$
For $x > 0$, $e^{-\frac{1}{x}} = e^{-\frac{1}{x}}$

Let's rewrite the integral as:
$\int_{-1}^1\frac{\cos x}{1+e^{-\frac{1}{x}}}\mathrm{d}x = \int_{-1}^0\frac{\cos x}{1+e^{\frac{1}{|x|}}}\mathrm{d}x + \int_0^1\frac{\cos x}{1+e^{-\frac{1}{x}}}\mathrm{d}x$

## Step 4: Use the symmetry of the interval
For the first integral, let's substitute $u = -x$:
$\int_{-1}^0\frac{\cos x}{1+e^{\frac{1}{|x|}}}\mathrm{d}x = \int_1^0\frac{\cos(-u)}{1+e^{\frac{1}{u}}}(-\mathrm{d}u) = \int_0^1\frac{\cos u}{1+e^{\frac{1}{u}}}\mathrm{d}u$

Now we have:
$\int_{-1}^1\frac{\cos x}{1+e^{-\frac{1}{x}}}\mathrm{d}x = \int_0^1\frac{\cos x}{1+e^{\frac{1}{x}}}\mathrm{d}x + \int_0^1\frac{\cos x}{1+e^{-\frac{1}{x}}}\mathrm{d}x$

## Step 5: Make a key observation
For any $x \neq 0$, note that:
$\frac{1}{1+e^{\frac{1}{x}}} + \frac{1}{1+e^{-\frac{1}{x}}} = \frac{1+e^{-\frac{1}{x}}}{(1+e^{\frac{1}{x}})(1+e^{-\frac{1}{x}})} + \frac{1+e^{\frac{1}{x}}}{(1+e^{\frac{1}{x}})(1+e^{-\frac{1}{x}})} = \frac{2+e^{\frac{1}{x}}+e^{-\frac{1}{x}}}{(1+e^{\frac{1}{x}})(1+e^{-\frac{1}{x}})} = 1$

So we have:
$\frac{1}{1+e^{\frac{1}{x}}} + \frac{1}{1+e^{-\frac{1}{x}}} = 1$

This means:
$\frac{1}{1+e^{\frac{1}{x}}} = 1 - \frac{1}{1+e^{-\frac{1}{x}}}$

## Step 6: Simplify the integral
Using this identity, we can rewrite our integral:
$\int_{-1}^1\frac{\cos x}{1+e^{-\frac{1}{x}}}\mathrm{d}x = \int_0^1\frac{\cos x}{1+e^{\frac{1}{x}}}\mathrm{d}x + \int_0^1\frac{\cos x}{1+e^{-\frac{1}{x}}}\mathrm{d}x$

$= \int_0^1\cos x\left(1-\frac{1}{1+e^{-\frac{1}{x}}}\right)\mathrm{d}x + \int_0^1\frac{\cos x}{1+e^{-\frac{1}{x}}}\mathrm{d}x$

$= \int_0^1\cos x\mathrm{d}x - \int_0^1\frac{\cos x}{1+e^{-\frac{1}{x}}}\mathrm{d}x + \int_0^1\frac{\cos x}{1+e^{-\frac{1}{x}}}\mathrm{d}x$

$= \int_0^1\cos x\mathrm{d}x = \sin x\big|_0^1 = \sin(1) - \sin(0) = \sin(1)$

## Step 7: Calculate the numerical value
The exact answer is $\sin(1)$.

The numerical approximation of $\sin(1)$ to 10 decimal places is 0.8414709848.

{"answer": "\\sin(1)", "numerical_answer": "0.8414709848"}