Let's compute the definite integral step by step.

### Step 1: Compute the integral analytically

The integral is:
\[
\int_{-1/2}^{1/2} \frac{dx}{1 - x^2}
\]

The integrand \(\frac{1}{1 - x^2}\) can be rewritten using partial fractions:
\[
\frac{1}{1 - x^2} = \frac{1}{(1 - x)(1 + x)} = \frac{1}{2} \left( \frac{1}{1 - x} + \frac{1}{1 + x} \right)
\]

Thus, the integral becomes:
\[
\int_{-1/2}^{1/2} \frac{dx}{1 - x^2} = \frac{1}{2} \left( \int_{-1/2}^{1/2} \frac{dx}{1 - x} + \int_{-1/2}^{1/2} \frac{dx}{1 + x} \right)
\]

Compute each integral separately:
\[
\int \frac{dx}{1 - x} = -\ln|1 - x| + C
\]
\[
\int \frac{dx}{1 + x} = \ln|1 + x| + C
\]

Now evaluate the definite integrals:
\[
\int_{-1/2}^{1/2} \frac{dx}{1 - x} = -\ln|1 - x| \Bigg|_{-1/2}^{1/2} = -\ln\left(\frac{1}{2}\right) + \ln\left(\frac{3}{2}\right) = \ln(3)
\]
\[
\int_{-1/2}^{1/2} \frac{dx}{1 + x} = \ln|1 + x| \Bigg|_{-1/2}^{1/2} = \ln\left(\frac{3}{2}\right) - \ln\left(\frac{1}{2}\right) = \ln(3)
\]

Combine the results:
\[
\int_{-1/2}^{1/2} \frac{dx}{1 - x^2} = \frac{1}{2} \left( \ln(3) + \ln(3) \right) = \frac{1}{2} \cdot 2 \ln(3) = \ln(3)
\]

### Step 2: Numerical approximation

The exact answer is \(\ln(3)\). Numerically:
\[
\ln(3) \approx 1.0986122887
\]

### Final answer in JSON format:
```json
{"answer": "\\ln(3)", "numerical_answer": "1.0986122887"}
```