Let's begin with the given integral:

\[
I = \int_{0}^{2} x^{-1/2}(2-x)^{-1/2} \arcsin\left(0.5\sqrt{x(2-x)}\right)\, dx
\]

**Step 1: Analytical Solution**

### 1. Substitution

Let us use the substitution:

Let \( x = 2\sin^2\theta \), where \( 0 \leq \theta \leq \frac{\pi}{2} \).
- When \( x = 0 \), \( \theta = 0 \).
- When \( x = 2 \), \( \sin^2\theta = 1 \implies \theta = \frac{\pi}{2} \).

Compute derivatives and useful expressions:

\[
dx = 4\sin\theta\cos\theta\, d\theta = 2\sin 2\theta\, d\theta
\]
\[
x^{-1/2} = \left(2\sin^2\theta\right)^{-1/2} = (2)^{-1/2} \sin^{-1}\theta
\]
\[
2-x = 2-2\sin^2\theta = 2\cos^2\theta \implies (2-x)^{-1/2} = (2)^{-1/2}\cos^{-1}\theta
\]
\[
\sqrt{x(2-x)} = \sqrt{2\sin^2\theta \cdot 2\cos^2\theta} = 2\sin\theta \cos\theta = \sin 2\theta
\]
So,
\[
0.5 \sqrt{x(2-x)} = 0.5 \cdot \sin 2\theta = \frac12 \sin 2\theta
\]

Now plug into the integral:

\[
I = \int_{x=0}^{x=2} x^{-1/2}(2-x)^{-1/2} \arcsin\left(0.5\sqrt{x(2-x)}\right)\, dx
\]
\[
= \int_{\theta=0}^{\theta=\pi/2} (2)^{-1} \sin^{-1}\theta \cos^{-1}\theta \cdot \arcsin\left( \frac12 \sin 2\theta \right) \cdot 2\sin 2\theta\, d\theta
\]
\[
= \int_{0}^{\pi/2} \frac1{2} \sin^{-1}\theta \cos^{-1}\theta \arcsin \left( \frac12 \sin 2\theta \right) 2\sin 2\theta \, d\theta
\]
\[
= \int_{0}^{\pi/2} \sin^{-1}\theta \cos^{-1}\theta \sin 2\theta \arcsin \left( \frac12 \sin 2\theta \right) d\theta
\]

But recall \( \sin^{-1}\theta \cos^{-1}\theta = \frac{1}{\sin\theta \cos\theta} \), but that's not what we have; we have the reciprocals, so let's just let it stand as written above.

In fact, from previous simplification:

\[
x^{-1/2} = \frac{1}{\sqrt{2}} \frac{1}{\sin\theta}
\]
\[
(2-x)^{-1/2} = \frac{1}{\sqrt{2}} \frac{1}{\cos\theta}
\]
\[
dx = 4\sin\theta\cos\theta\, d\theta
\]

So their product:
\[
x^{-1/2}(2-x)^{-1/2} dx = \frac{1}{2} \frac{1}{\sin\theta\cos\theta} 4\sin\theta\cos\theta\, d\theta = 2\, d\theta
\]

So the original integral simplifies greatly:

\[
I = \int_{0}^{2} x^{-1/2}(2-x)^{-1/2} \arcsin\left(0.5\sqrt{x(2-x)}\right)\, dx
= \int_{0}^{\pi/2} 2 \arcsin\left( \frac12 \sin 2\theta \right) d\theta
\]
\[
= 2 \int_0^{\pi/2} \arcsin\left( \frac12 \sin 2\theta \right) d\theta
\]

### 2. Further Analysis

Let \( \phi = 2\theta \implies d\phi = 2 d\theta \), when \( \theta = 0, \phi = 0 \), when \( \theta = \frac{\pi}{2}, \phi = \pi \):

\[
2 \int_{0}^{\pi/2} \arcsin \left( \frac12 \sin 2\theta \right) d\theta = 2 \cdot \int_{\theta=0}^{\theta=\pi/2} \arcsin\left( \frac12 \sin 2\theta \right) d\theta
\]
Let \( \phi = 2\theta \implies d\theta = \frac{d\phi}{2} \), \( \theta: 0 \to \frac{\pi}{2} \implies \phi: 0 \to \pi \):

\[
2 \int_0^{\pi/2} \arcsin\left( \frac12 \sin 2\theta \right) d\theta = 2 \int_{\phi=0}^{\phi=\pi} \arcsin\left( \frac12 \sin\phi \right) \frac{d\phi}{2}
= \int_0^{\pi} \arcsin\left( \frac12 \sin\phi \right) d\phi
\]

**So the integral reduces to:**

\[
I = \int_0^{\pi} \arcsin\left( \frac12 \sin\phi \right) d\phi
\]

### 3. Symmetry and Evaluation

Since \(\sin(\pi - \phi) = \sin\phi\), the integrand is even about \(\phi = \frac\pi2\). We can write:

\[
I = 2 \int_0^{\pi/2} \arcsin \left( \frac12 \sin\phi \right) d\phi
\]

But let's proceed with:
\[
I = \int_0^{\pi} \arcsin\left( \frac12 \sin\phi \right) d\phi
\]

#### Try Transforming the Sine

Recall that
\[
\arcsin\left( \frac12 \sin\phi \right)
\]
is somewhat tricky to integrate, but perhaps possible to express in terms of known constants.

#### Use Series Expansion

Alternatively, consider the Fourier expansion of \(\arcsin(a\sin\phi)\) for \(|a| \leq 1\):

It's a known identity:
\[
\arcsin(a\sin\phi) = \sum_{n=0}^\infty \frac{a^{2n+1}}{(2n+1)^2} \binom{2n}{n} \sin((2n+1)\phi) / 4^n
\]

So with \(a = \frac12\):

\[
\arcsin\left( \frac12 \sin\phi \right) = \sum_{n=0}^\infty \frac{ (\frac12)^{2n+1} }{ (2n+1)^2 } \binom{2n}{n} \frac{ \sin( (2n+1)\phi ) }{ 4^n }
\]

But \((\frac12)^{2n+1} / 4^n = (\frac12)^{2n+1 + 2n} = (\frac12)^{4n+1}\)

Wait, but more simply: \((\frac12)^{2n+1} / 4^n = (\frac12)^{2n+1} \cdot (4^{-n}) = (\frac12)^{2n+1} \cdot 2^{-2n} = 2^{-(2n+1+2n)} = 2^{-(4n+1)}\)

However, since 4^n = 2^{2n}, we have:

\[
\frac{ (\frac12)^{2n+1} }{ 4^n } = 2^{-(2n+1+2n)} = 2^{-(4n+1)}
\]

But \(\binom{2n}{n}\).

Thus:
\[
\arcsin\left( \frac12 \sin\phi \right) = \sum_{n=0}^\infty \frac{ \binom{2n}{n} }{ (2n+1)^2 2^{4n+1} } \sin((2n+1)\phi)
\]

Now, integrate over \(0\) to \(\pi\):

\[
I = \int_0^{\pi} \arcsin\left( \frac12 \sin\phi \right) d\phi = \sum_{n=0}^\infty \frac{ \binom{2n}{n} }{ (2n+1)^2 2^{4n+1} } \int_0^\pi \sin((2n+1)\phi) d\phi
\]

But
\[
\int_0^\pi \sin( (2n+1)\phi )\, d\phi = \left. -\frac{1}{2n+1} \cos((2n+1)\phi) \right|_0^\pi = -\frac{1}{2n+1}[\cos((2n+1)\pi) - \cos(0)]
\]
\[
\cos((2n+1)\pi) = -1,\ \cos(0) = 1 \implies -\frac{1}{2n+1}[ -1 - 1 ] = -\frac{1}{2n+1}[ -2 ] = \frac{2}{2n+1}
\]

So:
\[
I = \sum_{n=0}^\infty \frac{ \binom{2n}{n} }{ (2n+1)^2 2^{4n+1} } \cdot \frac{2}{2n+1 }
= \sum_{n=0}^\infty \frac{ \binom{2n}{n} }{ (2n+1)^3 2^{4n} }
\]

Recall \(2^{4n} = 16^n\):

\[
I = \sum_{n=0}^\infty \frac{ \binom{2n}{n} }{ (2n+1)^3 16^n }
\]

**This is the exact answer in closed form.**

---

**Step 2: Numerical Evaluation**

Let us compute the sum numerically, up to high order (say, \( n \) up to 20; the sum converges quickly):

For the first terms:
- \(n=0\): \( \binom{0}{0} = 1,\; (2n+1)^3 = 1 \), \( 16^0 = 1 \); term: \(1/1 = 1\)
- \(n=1\): \( \binom{2}{1} = 2,\; (2n+1)^3 = 3^3 = 27 \), \( 16^1 = 16 \); term: \( 2/(27 \times 16) = 2/432 = 1/216 \approx 0.0046296296 \)
- \(n=2\): \( \binom{4}{2} = 6,\; (5^3) = 125,\; 16^2 = 256 \); term: \(6/(125 \times 256 ) = 6/32000 = 0.0001875\)
- \(n=3\): \( \binom{6}{3} = 20,\; (7^3) = 343,\; 16^3=4096\); term: \( 20/(343\times4096) = 20/1404928 \approx 1.4245 \times 10^{-5}\)
- \(n=4\): \( \binom{8}{4} = 70, 9^3=729, 16^4=65536 \); \(70/(729 \times 65536) = 70 / 47775744 \approx 1.4646 \times 10^{-6}\)

Summing up:

- n=0: \( 1.0000000000 \)
- n=1: \( 0.0046296296 \)
- n=2: \( 0.0001875000 \)
- n=3: \( 0.0000142451 \)
- n=4: \( 0.0000014646 \)
- n=5: \( \binom{10}{5}=252,\; 11^3=1331,\; 16^5=1048576 \implies 252/(1331 \times 1048576) \approx 252/1395136256 \approx 1.8063\times10^{-7} \)
- n=6: \( \binom{12}{6}=924,\; 13^3=2197,\; 16^6=16777216; 924/(2197 \times 16777216)=924/36849979392 \approx 2.507\times10^{-8} \)

Add up the sum up to \( n=6 \):

Sum so far:
\[
1.0000000000
+0.0046296296
+0.0001875000
+0.0000142451
+0.0000014646
+0.0000001806
+0.0000000251
\]

\[
\approx 1.0048320450
\]

Additional terms will be much smaller, so truncating at this stage gives a numerical value accurate to at least 8 decimal places.

Thus:

\[
\boxed{1.0048320450}
\]

For more digits, use higher order, or a symbolic or numeric computation.

**Final Answers (in required JSON format):**

\[
\boxed{
\{"answer": "\sum_{n=0}^{\infty} \frac{\\binom{2n}{n}}{(2n+1)^3 16^n}", "numerical_answer": "1.0048320450"\}
}
\]