We begin with the integral

  I = ∫₀¹ [e^(eˣ) – e^(eˣ – x)] dx.

Step 1. Write I as the difference of two integrals:
  I = ∫₀¹ e^(eˣ) dx − ∫₀¹ e^(eˣ – x) dx.

Step 2. In the first integral let
  u = eˣ  ⇒ du = eˣ dx  ⇒ dx = du/u.
When x = 0, u = e⁰ = 1 and when x = 1, u = e.
Thus,
  ∫₀¹ e^(eˣ) dx = ∫₁ᵉ e^(u) (1/u) du = ∫₁ᵉ (e^(u)/u) du.
An antiderivative for e^(u)/u is given in terms of the exponential‐integral function Ei(u), but we shall soon see that a cancellation occurs.

Step 3. In the second integral write the integrand as
  e^(eˣ – x) = e^(eˣ)/eˣ.
Now make the same substitution u = eˣ, so that dx = du/u and when x runs from 0 to 1, u runs from 1 to e. Then
  ∫₀¹ e^(eˣ – x) dx = ∫₁ᵉ [e^(u)/u] (1/u) du = ∫₁ᵉ (e^(u)/u²) du.

Step 4. Thus our original integral becomes
  I = ∫₁ᵉ (e^(u)/u) du − ∫₁ᵉ (e^(u)/u²) du.
Notice that
  d/du (e^(u)/u) = (e^(u)·u − e^(u))/u² = e^(u)(u − 1)/u².
But in our difference the integrands “mesh” as follows. Write
  e^(u)/u − e^(u)/u² = [e^(u)(u − 1)]/u².
Thus,
  ∫₁ᵉ {e^(u)/u − e^(u)/u²} du = ∫₁ᵉ d/du (e^(u)/u) du.

So we immediately have
  I = [e^(u)/u]₍₁₎ᵉ = (e^(e)/e) − (e^(1)/1) = e^(e−1) − e.

Step 5. Final Answer.
The exact value of the integral is
  I = e^(e−1) − e.
A numerical approximation is found by using the approximate value e ≈ 2.7182818285. Then
  e^(e−1) = e^(1.7182818285) ≈ 5.5749145280,
so that
  I ≈ 5.5749145280 − 2.7182818285 ≈ 2.8566326995.

Thus, in the required JSON format the final answer is:
{"answer": "$e^{e-1}-e$", "numerical_answer": "2.8566326995"}