To solve the definite integral \(\int_0^1 (x-1)^2 (x+1)^2 (x^2+1)^2 (x^4+1)^2 \, dx\), we will follow the steps outlined:

### Step 1: Analytical Computation

First, let's expand the integrand \((x-1)^2 (x+1)^2 (x^2+1)^2 (x^4+1)^2\).

1. **Expand \((x-1)^2 (x+1)^2\):**
   \[
   (x-1)^2 (x+1)^2 = [(x-1)(x+1)]^2 = (x^2 - 1)^2 = x^4 - 2x^2 + 1
   \]

2. **Expand \((x^2+1)^2\):**
   \[
   (x^2+1)^2 = x^4 + 2x^2 + 1
   \]

3. **Expand \((x^4+1)^2\):**
   \[
   (x^4+1)^2 = x^8 + 2x^4 + 1
   \]

Now, we need to multiply these expanded forms together:
\[
(x^4 - 2x^2 + 1)(x^4 + 2x^2 + 1)(x^8 + 2x^4 + 1)
\]

Let's first multiply \((x^4 - 2x^2 + 1)\) and \((x^4 + 2x^2 + 1)\):
\[
(x^4 - 2x^2 + 1)(x^4 + 2x^2 + 1) = x^8 + 2x^6 + x^4 - 2x^6 - 4x^4 - 2x^2 + x^4 + 2x^2 + 1
\]
\[
= x^8 + (2x^6 - 2x^6) + (x^4 - 4x^4 + x^4) + (-2x^2 + 2x^2) + 1
\]
\[
= x^8 - 2x^4 + 1
\]

Next, multiply this result by \((x^8 + 2x^4 + 1)\):
\[
(x^8 - 2x^4 + 1)(x^8 + 2x^4 + 1) = x^{16} + 2x^{12} + x^8 - 2x^{12} - 4x^8 - 2x^4 + x^8 + 2x^4 + 1
\]
\[
= x^{16} + (2x^{12} - 2x^{12}) + (x^8 - 4x^8 + x^8) + (-2x^4 + 2x^4) + 1
\]
\[
= x^{16} - 2x^8 + 1
\]

Thus, the integrand simplifies to:
\[
(x-1)^2 (x+1)^2 (x^2+1)^2 (x^4+1)^2 = x^{16} - 2x^8 + 1
\]

### Step 2: Integrate Term-by-Term

Now, we integrate each term separately:
\[
\int_0^1 (x^{16} - 2x^8 + 1) \, dx = \int_0^1 x^{16} \, dx - 2 \int_0^1 x^8 \, dx + \int_0^1 1 \, dx
\]

1. **Integrate \(x^{16}\):**
   \[
   \int_0^1 x^{16} \, dx = \left[ \frac{x^{17}}{17} \right]_0^1 = \frac{1}{17}
   \]

2. **Integrate \(x^8\):**
   \[
   \int_0^1 x^8 \, dx = \left[ \frac{x^9}{9} \right]_0^1 = \frac{1}{9}
   \]

3. **Integrate \(1\):**
   \[
   \int_0^1 1 \, dx = \left[ x \right]_0^1 = 1
   \]

Combining these results:
\[
\int_0^1 (x^{16} - 2x^8 + 1) \, dx = \frac{1}{17} - 2 \cdot \frac{1}{9} + 1
\]
\[
= \frac{1}{17} - \frac{2}{9} + 1
\]

To combine these fractions, find a common denominator (153):
\[
\frac{1}{17} = \frac{9}{153}, \quad \frac{2}{9} = \frac{34}{153}, \quad 1 = \frac{153}{153}
\]
\[
\frac{9}{153} - \frac{34}{153} + \frac{153}{153} = \frac{9 - 34 + 153}{153} = \frac{128}{153}
\]

### Step 3: Numerical Approximation

The numerical approximation of \(\frac{128}{153}\) is:
\[
\frac{128}{153} \approx 0.8366013071895425
\]

### Step 4: Output the Final Answer

\[
\boxed{
\begin{aligned}
\text{"answer": "}\frac{128}{153}\text{"}, \\
\text{"numerical_answer": "0.8366013072"}
\end{aligned}
}
\]