# Evaluating $\int_{-1}^1 x^2 \cdot \sqrt[3]{x^3+1} \, dx$

I'll solve this definite integral using a substitution method.

## Step 1: Make a substitution
Let's set $u = x^3 + 1$, then $du = 3x^2 \, dx$, which means $x^2 \, dx = \frac{du}{3}$

When $x = -1$, $u = (-1)^3 + 1 = -1 + 1 = 0$
When $x = 1$, $u = 1^3 + 1 = 2$

So our integral becomes:
$$\int_{-1}^1 x^2 \cdot \sqrt[3]{x^3+1} \, dx = \int_{0}^2 \sqrt[3]{u} \cdot \frac{du}{3} = \frac{1}{3}\int_{0}^2 u^{1/3} \, du$$

## Step 2: Integrate $u^{1/3}$
$$\frac{1}{3}\int_{0}^2 u^{1/3} \, du = \frac{1}{3} \cdot \frac{u^{4/3}}{\frac{4}{3}} \bigg|_{0}^{2} = \frac{1}{4} \cdot u^{4/3} \bigg|_{0}^{2}$$

## Step 3: Evaluate at the bounds
$$\frac{1}{4} \cdot u^{4/3} \bigg|_{0}^{2} = \frac{1}{4} \cdot (2^{4/3} - 0^{4/3}) = \frac{1}{4} \cdot 2^{4/3} = \frac{2^{4/3}}{4}$$

## Step 4: Simplify
$$\frac{2^{4/3}}{4} = \frac{2^{4/3}}{2^2} = 2^{4/3-2} = 2^{4/3-6/3} = 2^{-2/3}$$

So the exact answer is $2^{-2/3}$.

## Step 5: Numerical approximation
$2^{-2/3} = \frac{1}{2^{2/3}} \approx 0.6299605249$

Therefore, $\int_{-1}^1 x^2 \cdot \sqrt[3]{x^3+1} \, dx = 2^{-2/3} \approx 0.6299605249$

{"answer": "2^{-2/3}", "numerical_answer": "0.6299605249"}