Let's proceed step by step:

### 1. Writing the integral clearly

We are given:
\[
I = \int_{1.0}^{\infty} x \left( x^2 - 1^2 \right)^{2 - \frac{3}{2}} e^{-0.5^2 x^2} H_{2\cdot2}(0.5x)\, dx
\]
This simplifies to:
\[
I = \int_1^\infty x (x^2-1)^{0.5} e^{-0.25 x^2} H_4(0.5x)\, dx
\]

### 2. Simplify and Substitute

#### Hermite polynomial \( H_4(z) \):
Recall:
\[
H_4(z) = 16z^4 - 48z^2 + 12
\]
Plug \( z = 0.5x \):
\[
H_4(0.5x) = 16(0.5x)^4 - 48(0.5x)^2 + 12 = 16 \cdot 0.0625 x^4 - 48 \cdot 0.25 x^2 + 12 = 1 x^4 - 12 x^2 + 12
\]

#### The integrand becomes:
\[
x(x^2-1)^{0.5} e^{-0.25 x^2} (x^4 - 12x^2 + 12)
\]

Therefore:

\[
I = \int_1^\infty x (x^2 - 1)^{0.5} e^{-0.25 x^2} (x^4 - 12x^2 + 12)\, dx
\]

### 3. Substitution

Let \( x = \cosh \theta \), \( \theta \in [0, \infty) \) when \( x \in [1, \infty) \), because \( \cosh 0 = 1 \).
Then:
- \( x^2 - 1 = \sinh^2 \theta \)
- \( (x^2-1)^{0.5} = \sinh \theta \)
- \( dx = \sinh \theta\, d\theta \)
- \( x = \cosh \theta \)

The bounds:
- When \( x=1 \Rightarrow \theta=0 \)
- When \( x\to\infty \Rightarrow \theta\to\infty \)

Substitute into the integral:
\[
I = \int_0^\infty \cosh \theta \cdot \sinh \theta\, e^{-0.25 \cosh^2\theta} \left( (\cosh\theta)^4 - 12 (\cosh\theta)^2 + 12 \right) \sinh\theta\, d\theta
\]

Combine like terms:
- \( \cosh\theta \cdot \sinh\theta \cdot \sinh\theta = \cosh\theta \cdot \sinh^2\theta \)

So:
\[
I = \int_0^\infty \cosh\theta\, \sinh^2\theta\, e^{-0.25\cosh^2\theta} \left( (\cosh\theta)^4 - 12 (\cosh\theta)^2 + 12 \right) d\theta
\]

But let's expand \( \sinh^2\theta \):
\[
\sinh^2\theta = \cosh^2\theta - 1
\]
So:
\[
\cosh\theta \cdot \sinh^2\theta = \cosh\theta (\cosh^2\theta - 1) = \cosh^3\theta - \cosh\theta
\]

Therefore:
\[
I = \int_0^\infty (\cosh^3\theta - \cosh\theta) e^{-0.25\cosh^2\theta} \left((\cosh\theta)^4 - 12(\cosh\theta)^2 + 12 \right) d\theta
\]

Expand the product:
Let \( A = \cosh^3\theta - \cosh\theta \)
Let \( B = (\cosh\theta)^4 - 12(\cosh\theta)^2 + 12 \)

Compute \( A \cdot B \):

Let \( C = \cosh\theta \)

\[
A \cdot B = (C^3 - C)(C^4 - 12C^2 + 12) = C^3 (C^4 - 12C^2 + 12) - C(C^4 - 12C^2 + 12)
\]
\[
= C^7 - 12C^5 + 12C^3 - C^5 + 12C^3 - 12C
\]
\[
= C^7 - 12C^5 + 12C^3 - C^5 + 12C^3 - 12C
\]
\[
= C^7 - (12+1) C^5 + (12+12)C^3 - 12C
\]
\[
= C^7 - 13C^5 + 24C^3 - 12C
\]

So finally:
\[
I = \int_0^\infty \left(\cosh^7\theta - 13\cosh^5\theta + 24\cosh^3\theta - 12\cosh\theta \right) e^{-0.25\cosh^2\theta} d\theta
\]

### 4. Back-substitution (Optional)

Alternatively, this can be written as the sum of four integrals:

\[
I = \int_0^\infty \cosh^7\theta\, e^{-0.25\cosh^2\theta} d\theta
- 13 \int_0^\infty \cosh^5\theta\, e^{-0.25\cosh^2\theta} d\theta
+ 24 \int_0^\infty \cosh^3\theta\, e^{-0.25\cosh^2\theta} d\theta
- 12 \int_0^\infty \cosh\theta\, e^{-0.25\cosh^2\theta} d\theta
\]

Alternatively, let's consider going back to the original variable for a cleaner analytic form.

### 5. Try a Substitution \( u = x^2 \)

Let \( u = x^2 \), \( x = \sqrt{u} \), \( dx = \frac{du}{2\sqrt{u}} \), \( x^2-1 = u-1 \).
The bounds: \( x=1 \rightarrow u=1 \), \( x\to\infty \rightarrow u\to\infty \).

Original integrand:
\[
x(x^2-1)^{0.5} e^{-0.25 x^2} (x^4 - 12x^2 + 12)\, dx
\]
Substitute:
- \( x = \sqrt{u} \)
- \( x^2-1 = u-1 \)
- \( (x^2-1)^{0.5} = (u-1)^{0.5} \)
- \( x^4 - 12x^2 + 12 = u^2 - 12u + 12 \)
- \( dx = \frac{du}{2\sqrt{u}} \)

Now,
\[
x(x^2-1)^{0.5} (x^4 - 12x^2 + 12)\, dx = \sqrt{u}(u-1)^{0.5}(u^2 - 12u + 12)\,\frac{du}{2\sqrt{u}}
\]
\[
= \frac{1}{2} (u-1)^{0.5}(u^2 - 12u + 12)\, du
\]

Hence,
\[
I = \frac{1}{2} \int_{u=1}^\infty (u-1)^{0.5} (u^2 - 12u + 12) e^{-0.25u} du
\]

### 6. This has a standard form

Let's separate the polynomial:

\[
I = \frac{1}{2} \int_1^\infty (u-1)^{0.5} u^2 e^{-0.25u} du
 - 6 \int_1^\infty (u-1)^{0.5} u e^{-0.25u} du
 + 6 \int_1^\infty (u-1)^{0.5} e^{-0.25u} du
\]

### 7. Substitution \( t = u-1 \implies u = t+1, du = dt\)

When \( u = 1 \), \( t = 0 \), when \( u\to\infty, t\to\infty \).

Now,
- \( (u-1)^{0.5} = t^{0.5} \)
- \( u^2 = (t+1)^2 = t^2 + 2t + 1 \)
- \( u = t+1 \)
- \( e^{-0.25u} = e^{-0.25 t} e^{-0.25} \)

Plug in:

First term:
\[
\int_1^\infty (u-1)^{0.5} u^2 e^{-0.25u}\, du
= \int_0^\infty t^{0.5} (t+1)^2 e^{-0.25t} e^{-0.25} dt
\]
\[
= e^{-0.25} \int_0^\infty t^{0.5} (t^2 + 2t + 1) e^{-0.25 t} dt
\]
\[
= e^{-0.25} \left( \int_0^\infty t^{2.5} e^{-0.25 t} dt + 2\int_0^\infty t^{1.5} e^{-0.25 t} dt + \int_0^\infty t^{0.5} e^{-0.25 t} dt \right)
\]

Similarly for the other terms:

Second term:
\[
-12 \int_1^\infty (u-1)^{0.5} u e^{-0.25u} du
= -12 e^{-0.25} \int_0^\infty t^{0.5} (t+1) e^{-0.25 t} dt
\]
\[
= -12 e^{-0.25} \left( \int_0^\infty t^{1.5} e^{-0.25 t} dt + \int_0^\infty t^{0.5} e^{-0.25 t} dt \right)
\]

Third term:
\[
+12 \int_1^\infty (u-1)^{0.5} e^{-0.25u} du
= 12 e^{-0.25} \int_0^\infty t^{0.5} e^{-0.25 t} dt
\]

Now, combine all terms:

First, collect all common terms:

- \( I_1 = \int_0^\infty t^{2.5} e^{-0.25 t} dt \)
- \( I_2 = \int_0^\infty t^{1.5} e^{-0.25 t} dt \)
- \( I_3 = \int_0^\infty t^{0.5} e^{-0.25 t} dt \)

Plug in coefficients:

- \( I \) is:

\[
I = \frac{1}{2} e^{-0.25} \Bigg[
I_1 + 2 I_2 + I_3 - 12(I_2 + I_3) + 12 I_3
\Bigg]
\]

Expand:

- \( I_2 \): \( +2I_2 - 12I_2 = -10I_2 \)
- \( I_3 \): \( +I_3 -12I_3 +12I_3 = +I_3 \)
- So, \( +I_3 \) remains.

So,
\[
I = \frac{1}{2} e^{-0.25}\, (I_1 - 10I_2 + I_3 )
\]

### 8. Express the integrals using the Gamma function

Recall,
\[
\int_0^\infty t^{k} e^{-at} dt = \frac{\Gamma(k+1)}{a^{k+1}}
\]

Set \( a=0.25 \)

- \( I_1 = \int_0^\infty t^{2.5} e^{-0.25 t} dt = \frac{\Gamma(3.5)}{0.25^{3.5}} \)
- \( I_2 = \int_0^\infty t^{1.5} e^{-0.25 t} dt = \frac{\Gamma(2.5)}{0.25^{2.5}} \)
- \( I_3 = \int_0^\infty t^{0.5} e^{-0.25 t} dt = \frac{\Gamma(1.5)}{0.25^{1.5}} \)

So,
\[
I = \frac{1}{2} e^{-0.25} \left[ \frac{\Gamma(3.5)}{0.25^{3.5}} - 10 \frac{\Gamma(2.5)}{0.25^{2.5}} + \frac{\Gamma(1.5)}{0.25^{1.5}} \right]
\]

This is the exact analytic answer.

### 9. Simplifying \( 0.25^{n} \)

Recall \( 0.25 = 1/4 \).

So,
- \( 0.25^{3.5} = (1/4)^{3.5} = 4^{-3.5} = 2^{-7} = 1/128 \)
- \( 0.25^{2.5} = (1/4)^{2.5} = 4^{-2.5} = 2^{-5} = 1/32 \)
- \( 0.25^{1.5} = (1/4)^{1.5} = 4^{-1.5} = 2^{-3} = 1/8 \)

Also, the Gamma values:
- \( \Gamma(1.5) = \frac{1}{2} \sqrt{\pi} \)
- \( \Gamma(2.5) = \frac{3}{4} \sqrt{\pi} \)
- \( \Gamma(3.5) = \frac{3}{4} \cdot \frac{5}{2} \sqrt{\pi} = \frac{15}{8} \sqrt{\pi} \)

### 10. Substitute these:

So,
\[
I = \frac{1}{2} e^{-0.25} \left[ 128 \cdot \Gamma(3.5) - 10 \times 32 \cdot \Gamma(2.5) + 8 \cdot \Gamma(1.5) \right]
\]

Now substitute Gamma values:
- \( 128 \cdot \Gamma(3.5) = 128 \cdot \frac{15}{8} \sqrt{\pi} = 16 \cdot 15 \sqrt{\pi} = 240 \sqrt{\pi} \)
- \( 10 \times 32 \cdot \Gamma(2.5) = 320 \cdot \frac{3}{4} \sqrt{\pi} = 80 \cdot 3 \sqrt{\pi} = 240 \sqrt{\pi} \)
- \( 8 \cdot \Gamma(1.5) = 8 \cdot \frac{1}{2} \sqrt{\pi} = 4 \sqrt{\pi} \)

So,
\[
I = \frac{1}{2} e^{-0.25} \left[ 240 \sqrt{\pi} - 240 \sqrt{\pi} + 4\sqrt{\pi} \right] = \frac{1}{2} e^{-0.25} (4\sqrt{\pi})
= 2 \sqrt{\pi} e^{-0.25}
\]

**This is the exact, fully simplified answer!**

### 11. Numerical Approximation

- \( \sqrt{\pi} \approx 1.7724538509 \)
- \( e^{-0.25} \approx 0.7788007831 \)

Therefore,
\[
I \approx 2 \cdot 1.7724538509 \cdot 0.7788007831 \approx 2 \cdot 1.3783996121 \approx 2.7567992242
\]

Thus, rounded to 10 decimal places:
\[
I \approx 2.7567992242
\]

---

### 12. Final JSON Output

```json
{"answer": "2 \\sqrt{\\pi} e^{-0.25}", "numerical_answer": "2.7567992242"}
```