Let's proceed step by step.

## 1. Understanding the Integral

We are to compute:
\[
I = \int_0^1 x \, \mathbf{L}_0(2\sqrt{x}) \, \mathbf{K}\left(\sqrt{1-x}\right) dx
\]
where:
- \(\mathbf{L}_0(z)\) is the modified Struve function of order 0,
- \(\mathbf{K}(k)\) is the complete elliptic integral of the first kind.

## 2. Substitution

Let us try the substitution \(x = t^2\), so \(dx = 2t\,dt\), \(x \in [0,1] \implies t \in [0,1]\):

\[
I = \int_{t=0}^{1} (t^2) \mathbf{L}_0(2t) \mathbf{K}(\sqrt{1-t^2}) \cdot 2t\,dt
= 2 \int_0^1 t^3 \mathbf{L}_0(2t) \mathbf{K}(\sqrt{1-t^2}) dt
\]

Now, recall that \(\mathbf{K}(\sqrt{1-t^2}) = \int_0^{\pi/2} \frac{d\theta}{\sqrt{1 - (1-t^2)\sin^2\theta}} = \int_0^{\pi/2} \frac{d\theta}{\sqrt{t^2\sin^2\theta + \cos^2\theta}}\).

But let's see if we can relate this to a known integral.

## 3. Series Expansion for \(\mathbf{L}_0(2t)\)

The modified Struve function of order 0 has the series:
\[
\mathbf{L}_0(z) = \sum_{m=0}^\infty \frac{(z/2)^{2m+1}}{\Gamma(m+\frac{3}{2}) \Gamma(m+1)}
\]
So,
\[
\mathbf{L}_0(2t) = \sum_{m=0}^\infty \frac{t^{2m+1}}{\Gamma(m+\frac{3}{2}) \Gamma(m+1)}
\]

Therefore,
\[
t^3 \mathbf{L}_0(2t) = \sum_{m=0}^\infty \frac{t^{2m+4}}{\Gamma(m+\frac{3}{2}) \Gamma(m+1)}
\]

So,
\[
I = 2 \int_0^1 \left( \sum_{m=0}^\infty \frac{t^{2m+4}}{\Gamma(m+\frac{3}{2}) \Gamma(m+1)} \right) \mathbf{K}(\sqrt{1-t^2}) dt
= 2 \sum_{m=0}^\infty \frac{1}{\Gamma(m+\frac{3}{2}) \Gamma(m+1)} \int_0^1 t^{2m+4} \mathbf{K}(\sqrt{1-t^2}) dt
\]

## 4. Integral Representation for \(\mathbf{K}(\sqrt{1-t^2})\)

Recall:
\[
\int_0^1 t^n \mathbf{K}(\sqrt{1-t^2}) dt = \frac{\sqrt{\pi}}{2} \frac{\Gamma\left(\frac{n+1}{2}\right)}{\Gamma\left(\frac{n}{2}+1\right)}
\]
(see Gradshteyn & Ryzhik 3.147.2)

So for \(n = 2m+4\):
\[
\int_0^1 t^{2m+4} \mathbf{K}(\sqrt{1-t^2}) dt = \frac{\sqrt{\pi}}{2} \frac{\Gamma(m+2.5)}{\Gamma(m+3)}
\]

## 5. Substitute Back

So,
\[
I = 2 \sum_{m=0}^\infty \frac{1}{\Gamma(m+\frac{3}{2}) \Gamma(m+1)} \cdot \frac{\sqrt{\pi}}{2} \frac{\Gamma(m+2.5)}{\Gamma(m+3)}
= \sqrt{\pi} \sum_{m=0}^\infty \frac{\Gamma(m+2.5)}{\Gamma(m+\frac{3}{2}) \Gamma(m+1) \Gamma(m+3)}
\]

Now, recall that \(\Gamma(m+2.5) = (m+1.5)(m+0.5)\Gamma(m+0.5)\), and \(\Gamma(m+3) = (m+2)(m+1)\Gamma(m+1)\).

But let's try to simplify the ratio:
\[
\frac{\Gamma(m+2.5)}{\Gamma(m+3)} = \frac{(m+2.5-1)\Gamma(m+1.5)}{(m+3-1)\Gamma(m+2)} = \frac{(m+1.5)\Gamma(m+1.5)}{(m+2)\Gamma(m+2)}
\]
But \(\Gamma(m+2) = (m+1)\Gamma(m+1)\), so
\[
\frac{\Gamma(m+2.5)}{\Gamma(m+3)} = \frac{(m+1.5)\Gamma(m+1.5)}{(m+2)(m+1)\Gamma(m+1)}
\]

So the sum becomes:
\[
I = \sqrt{\pi} \sum_{m=0}^\infty \frac{(m+1.5)\Gamma(m+1.5)}{\Gamma(m+\frac{3}{2}) \Gamma(m+1) (m+2)(m+1)\Gamma(m+1)}
\]
But \(\Gamma(m+1.5) = \Gamma(m+\frac{3}{2})\), so
\[
I = \sqrt{\pi} \sum_{m=0}^\infty \frac{m+1.5}{(m+2)(m+1)[\Gamma(m+1)]^2}
\]

Let us write \(m+1.5 = m+3/2\), \(m+2 = m+2\), \(m+1 = m+1\):

\[
I = \sqrt{\pi} \sum_{m=0}^\infty \frac{m+\frac{3}{2}}{(m+2)(m+1)[\Gamma(m+1)]^2}
\]

But \(\Gamma(m+1) = m!\), so
\[
I = \sqrt{\pi} \sum_{m=0}^\infty \frac{m+\frac{3}{2}}{(m+2)(m+1)[m!]^2}
\]

## 6. Final Exact Answer

Thus, the exact answer is:
\[
I = \sqrt{\pi} \sum_{m=0}^\infty \frac{m+\frac{3}{2}}{(m+2)(m+1)[m!]^2}
\]

## 7. Numerical Approximation

Let us compute the first few terms:

For \(m=0\):
\[
\frac{0+1.5}{(0+2)(0+1)[0!]^2} = \frac{1.5}{2 \cdot 1 \cdot 1} = 0.75
\]

For \(m=1\):
\[
\frac{1+1.5}{(1+2)(1+1)[1!]^2} = \frac{2.5}{3 \cdot 2 \cdot 1} = \frac{2.5}{6} \approx 0.4166666667
\]

For \(m=2\):
\[
\frac{2+1.5}{(2+2)(2+1)[2!]^2} = \frac{3.5}{4 \cdot 3 \cdot 4} = \frac{3.5}{48} \approx 0.0729166667
\]

For \(m=3\):
\[
\frac{3+1.5}{(3+2)(3+1)[3!]^2} = \frac{4.5}{5 \cdot 4 \cdot 36} = \frac{4.5}{720} = 0.00625
\]

For \(m=4\):
\[
\frac{4+1.5}{(4+2)(4+1)[4!]^2} = \frac{5.5}{6 \cdot 5 \cdot 576} = \frac{5.5}{17280} \approx 0.0003182870
\]

For \(m=5\):
\[
\frac{5+1.5}{(5+2)(5+1)[5!]^2} = \frac{6.5}{7 \cdot 6 \cdot 14400} = \frac{6.5}{604800} \approx 0.0000107513
\]

Sum of first 6 terms:
\[
S_5 = 0.75 + 0.4166666667 + 0.0729166667 + 0.00625 + 0.0003182870 + 0.0000107513 \approx 1.246162371
\]

Multiply by \(\sqrt{\pi} \approx 1.7724538509\):

\[
I \approx 1.7724538509 \times 1.246162371 \approx 2.210370393
\]

Let's add a few more terms for accuracy:

For \(m=6\):
\[
\frac{7.5}{8 \cdot 7 \cdot 518400} = \frac{7.5}{29030400} \approx 0.0000002584
\]

For \(m=7\):
\[
\frac{8.5}{9 \cdot 8 \cdot 25401600} = \frac{8.5}{1830115200} \approx 0.0000000046
\]

So the sum converges rapidly. Adding these, the sum is about \(1.246162633\), so

\[
I \approx 1.7724538509 \times 1.246162633 \approx 2.210370789
\]

Rounding to 10 decimal places:

\[
I \approx 2.2103707890
\]

## 8. Final JSON Output

```json
{"answer": "\\sqrt{\\pi} \\sum_{m=0}^\\infty \\frac{m+\\frac{3}{2}}{(m+2)(m+1)[m!]^2}", "numerical_answer": "2.2103707890"}
```