# Evaluating $\int_0^{\frac{\pi}{4}}\tan^{-1}\left(\frac{1+\tan(x)}{\sqrt{2}}\right)\mathrm{d}x$

## Step 1: Simplify the integrand

Let's make a substitution to simplify the expression. Let $u = \tan(x)$, which means:
- $x = \tan^{-1}(u)$
- $dx = \frac{1}{1+u^2}du$
- When $x = 0$, $u = 0$
- When $x = \frac{\pi}{4}$, $u = 1$

So our integral becomes:
$$\int_0^{1}\tan^{-1}\left(\frac{1+u}{\sqrt{2}}\right)\frac{1}{1+u^2}du$$

## Step 2: Manipulate the arctangent expression

Let's examine the expression $\tan^{-1}\left(\frac{1+u}{\sqrt{2}}\right)$.

We can use the identity: $\tan^{-1}(a) + \tan^{-1}(b) = \tan^{-1}\left(\frac{a+b}{1-ab}\right)$ when $ab < 1$

Let's try to express $\frac{1+u}{\sqrt{2}}$ in a form that allows us to use this identity.

Consider $\tan^{-1}\left(\frac{1}{\sqrt{2}}\right) + \tan^{-1}\left(\frac{u}{\sqrt{2}}\right)$:

$\tan^{-1}\left(\frac{1}{\sqrt{2}}\right) + \tan^{-1}\left(\frac{u}{\sqrt{2}}\right) = \tan^{-1}\left(\frac{\frac{1}{\sqrt{2}}+\frac{u}{\sqrt{2}}}{1-\frac{1}{\sqrt{2}}\cdot\frac{u}{\sqrt{2}}}\right) = \tan^{-1}\left(\frac{\frac{1+u}{\sqrt{2}}}{1-\frac{u}{2}}\right)$

This isn't exactly what we want. Let's try a different approach.

We know that $\tan^{-1}\left(\frac{1}{\sqrt{2}}\right) = \frac{\pi}{8}$ (since $\tan(\frac{\pi}{8}) = \frac{1}{\sqrt{2}}$)

Let's substitute $v = \frac{1+u}{\sqrt{2}}$. Then:
- When $u = 0$, $v = \frac{1}{\sqrt{2}}$
- When $u = 1$, $v = \frac{2}{\sqrt{2}} = \sqrt{2}$
- $u = \sqrt{2}v - 1$
- $du = \sqrt{2}dv$

So our integral becomes:
$$\int_{\frac{1}{\sqrt{2}}}^{\sqrt{2}}\tan^{-1}(v)\frac{\sqrt{2}}{1+(\sqrt{2}v-1)^2}dv$$

## Step 3: Use a more direct approach

Let's start fresh with a substitution $t = \frac{1+\tan(x)}{\sqrt{2}}$

When $x = 0$, $t = \frac{1}{\sqrt{2}}$
When $x = \frac{\pi}{4}$, $t = \frac{1+1}{\sqrt{2}} = \frac{2}{\sqrt{2}} = \sqrt{2}$

From $t = \frac{1+\tan(x)}{\sqrt{2}}$, we get $\tan(x) = \sqrt{2}t - 1$
Therefore, $\frac{dx}{dt} = \frac{1}{1+\tan^2(x)} \cdot \frac{d\tan(x)}{dt} = \frac{1}{1+(\sqrt{2}t-1)^2} \cdot \sqrt{2}$

Our integral becomes:
$$\int_{\frac{1}{\sqrt{2}}}^{\sqrt{2}}\tan^{-1}(t)\frac{dt}{\sqrt{2}} = \frac{1}{\sqrt{2}}\int_{\frac{1}{\sqrt{2}}}^{\sqrt{2}}\tan^{-1}(t)dt$$

We can use integration by parts with:
- $u = \tan^{-1}(t)$
- $dv = dt$
- $du = \frac{1}{1+t^2}dt$
- $v = t$

$$\frac{1}{\sqrt{2}}\left[t\tan^{-1}(t) - \int_{\frac{1}{\sqrt{2}}}^{\sqrt{2}} \frac{t}{1+t^2}dt\right]$$

For the remaining integral:
$$\int \frac{t}{1+t^2}dt = \frac{1}{2}\ln(1+t^2)$$

So our result is:
$$\frac{1}{\sqrt{2}}\left[t\tan^{-1}(t) - \frac{1}{2}\ln(1+t^2)\right]_{\frac{1}{\sqrt{2}}}^{\sqrt{2}}$$

Evaluating at the limits:
$$\frac{1}{\sqrt{2}}\left[\sqrt{2}\tan^{-1}(\sqrt{2}) - \frac{1}{2}\ln(1+2) - \frac{1}{\sqrt{2}}\tan^{-1}\left(\frac{1}{\sqrt{2}}\right) + \frac{1}{2}\ln\left(1+\frac{1}{2}\right)\right]$$

We know:
- $\tan^{-1}(\sqrt{2}) = \frac{3\pi}{8}$
- $\tan^{-1}\left(\frac{1}{\sqrt{2}}\right) = \frac{\pi}{8}$

Substituting:
$$\frac{1}{\sqrt{2}}\left[\sqrt{2}\cdot\frac{3\pi}{8} - \frac{1}{2}\ln(3) - \frac{1}{\sqrt{2}}\cdot\frac{\pi}{8} + \frac{1}{2}\ln\left(\frac{3}{2}\right)\right]$$

$$\frac{1}{\sqrt{2}}\left[\frac{3\pi}{4} - \frac{\pi}{8\sqrt{2}} - \frac{1}{2}\ln(3) + \frac{1}{2}\ln\left(\frac{3}{2}\right)\right]$$

$$\frac{1}{\sqrt{2}}\left[\frac{3\pi}{4} - \frac{\pi}{8\sqrt{2}} - \frac{1}{2}\ln\left(\frac{3}{\frac{3}{2}}\right)\right]$$

$$\frac{1}{\sqrt{2}}\left[\frac{3\pi}{4} - \frac{\pi}{8\sqrt{2}} - \frac{1}{2}\ln(2)\right]$$

Simplifying:
$$\frac{3\pi}{4\sqrt{2}} - \frac{\pi}{8(\sqrt{2})^2} - \frac{\ln(2)}{2\sqrt{2}} = \frac{3\pi}{4\sqrt{2}} - \frac{\pi}{16} - \frac{\ln(2)}{2\sqrt{2}}$$

## Step 4: Final simplification and numerical calculation

The exact answer is:
$$\frac{3\pi}{4\sqrt{2}} - \frac{\pi}{16} - \frac{\ln(2)}{2\sqrt{2}}$$

Numerically, this equals:
- $\frac{3\pi}{4\sqrt{2}} ≈ 1.6632526142$
- $\frac{\pi}{16} ≈ 0.1963495408$
- $\frac{\ln(2)}{2\sqrt{2}} ≈ 0.2402265070$

Therefore, $\frac{3\pi}{4\sqrt{2}} - \frac{\pi}{16} - \frac{\ln(2)}{2\sqrt{2}} ≈ 1.2266765664$

{"answer": "\\frac{3\\pi}{4\\sqrt{2}} - \\frac{\\pi}{16} - \\frac{\\ln(2)}{2\\sqrt{2}}", "numerical_answer": "1.2266765664"}