Let's denote the integral:
\[
I = \int_{-1}^1 \frac{\cos x}{1+e^{-1/x}}\,dx.
\]

**Step 1: Analyze the symmetry and substitution**

Let’s try the substitution \( x \mapsto -x \):

\[
I = \int_{-1}^1 \frac{\cos x}{1+e^{-1/x}}\,dx = \int_{-1}^1 \frac{\cos(-x)}{1+e^{-1/(-x)}}\,dx
\]
Since \(\cos(-x) = \cos x\) and \(1/(-x) = -1/x\), so:

\[
e^{-1/(-x)} = e^{1/x}
\]
So denoting \( f(x) = \frac{\cos x}{1+e^{-1/x}} \), our substitution gives:

\[
f(-x) = \frac{\cos x}{1 + e^{1/x}}
\]
So,
\[
I = \int_{-1}^1 \frac{\cos x}{1+e^{-1/x}}\,dx = \int_{-1}^1 \frac{\cos x}{1+e^{1/x}}\,dx
\]

Add both expressions:

\[
2I = \int_{-1}^1 \left(\frac{\cos x}{1+e^{-1/x}} + \frac{\cos x}{1+e^{1/x}} \right) dx
\]

Combine fractions:

\[
\frac{\cos x}{1+e^{-1/x}} + \frac{\cos x}{1+e^{1/x}} = \cos x\left( \frac{1}{1+e^{-1/x}} + \frac{1}{1+e^{1/x}} \right)
\]

\[
= \cos x \left( \frac{1+e^{1/x}+1+e^{-1/x}}{(1+e^{-1/x})(1+e^{1/x})} \right)
\]

Let’s compute the denominator:

\[
(1+e^{-1/x})(1+e^{1/x}) = 1 + e^{1/x} + e^{-1/x} + 1 = 2 + e^{1/x} + e^{-1/x}
\]

Similarly, the numerator:

\[
1 + e^{1/x} + 1 + e^{-1/x} = 2 + e^{1/x} + e^{-1/x}
\]

Therefore:

\[
\frac{1}{1+e^{-1/x}} + \frac{1}{1+e^{1/x}} = \frac{2 + e^{1/x} + e^{-1/x}}{2 + e^{1/x} + e^{-1/x}} = 1
\]

Therefore:

\[
2I = \int_{-1}^1 \cos x\, dx
\]

So,

\[
I = \frac{1}{2} \int_{-1}^1 \cos x\, dx
\]

**Step 2: Calculate the final integral**

We know:
\[
\int_{-1}^1 \cos x\, dx = [\sin x]_{-1}^1 = \sin 1 - \sin (-1) = \sin 1 + \sin 1 = 2\sin 1
\]

Therefore:
\[
I = \frac{1}{2} \times 2\sin 1 = \sin 1
\]

**Step 3: Numerical value**

To 10 decimal places:
\[
\sin 1\ \approx\ 0.8414709848
\]

**Step 4: JSON output**

```json
{"answer": "\\sin 1", "numerical_answer": "0.8414709848"}
```