To solve the definite integral \(\int_0^1 \frac{e^{\arctan(x)}}{(x^2+1)^{3/2}} \, dx\), we will follow the steps outlined.

### Step 1: Analytical Solution

First, let's make a substitution to simplify the integral. Let \( t = \arctan(x) \). Then, \( x = \tan(t) \) and \( dx = \sec^2(t) \, dt \).

The limits of integration change as follows:
- When \( x = 0 \), \( t = \arctan(0) = 0 \).
- When \( x = 1 \), \( t = \arctan(1) = \frac{\pi}{4} \).

The integral becomes:
\[
\int_0^{\frac{\pi}{4}} \frac{e^t}{(\tan^2(t) + 1)^{3/2}} \sec^2(t) \, dt
\]

Since \(\tan^2(t) + 1 = \sec^2(t)\), we have:
\[
(\tan^2(t) + 1)^{3/2} = (\sec^2(t))^{3/2} = \sec^3(t)
\]

Thus, the integral simplifies to:
\[
\int_0^{\frac{\pi}{4}} \frac{e^t}{\sec^3(t)} \sec^2(t) \, dt = \int_0^{\frac{\pi}{4}} e^t \cos(t) \, dt
\]

Now, we need to evaluate \(\int e^t \cos(t) \, dt\). We use integration by parts. Let:
\[
u = e^t \quad \text{and} \quad dv = \cos(t) \, dt
\]
Then:
\[
du = e^t \, dt \quad \text{and} \quad v = \sin(t)
\]

Using integration by parts:
\[
\int e^t \cos(t) \, dt = e^t \sin(t) - \int e^t \sin(t) \, dt
\]

We need to evaluate \(\int e^t \sin(t) \, dt\) again by parts. Let:
\[
u = e^t \quad \text{and} \quad dv = \sin(t) \, dt
\]
Then:
\[
du = e^t \, dt \quad \text{and} \quad v = -\cos(t)
\]

Using integration by parts again:
\[
\int e^t \sin(t) \, dt = -e^t \cos(t) + \int e^t \cos(t) \, dt
\]

Let \( I = \int e^t \cos(t) \, dt \). Then:
\[
I = e^t \sin(t) - (-e^t \cos(t) + I)
\]
\[
I = e^t \sin(t) + e^t \cos(t) - I
\]
\[
2I = e^t (\sin(t) + \cos(t))
\]
\[
I = \frac{e^t (\sin(t) + \cos(t))}{2}
\]

Thus:
\[
\int_0^{\frac{\pi}{4}} e^t \cos(t) \, dt = \left[ \frac{e^t (\sin(t) + \cos(t))}{2} \right]_0^{\frac{\pi}{4}}
\]

Evaluating at the limits:
\[
\left[ \frac{e^{\frac{\pi}{4}} (\sin(\frac{\pi}{4}) + \cos(\frac{\pi}{4}))}{2} \right] - \left[ \frac{e^0 (\sin(0) + \cos(0))}{2} \right]
\]

Since \(\sin(\frac{\pi}{4}) = \cos(\frac{\pi}{4}) = \frac{\sqrt{2}}{2}\) and \(\sin(0) = 0\), \(\cos(0) = 1\):
\[
\left[ \frac{e^{\frac{\pi}{4}} (\frac{\sqrt{2}}{2} + \frac{\sqrt{2}}{2})}{2} \right] - \left[ \frac{1 (0 + 1)}{2} \right]
\]
\[
= \left[ \frac{e^{\frac{\pi}{4}} \sqrt{2}}{2} \right] - \left[ \frac{1}{2} \right]
\]
\[
= \frac{e^{\frac{\pi}{4}} \sqrt{2}}{2} - \frac{1}{2}
\]

### Step 2: Numerical Approximation

Using a calculator to approximate the numerical value:
\[
e^{\frac{\pi}{4}} \approx 2.1932800507380155
\]
\[
\frac{2.1932800507380155 \cdot \sqrt{2}}{2} \approx 1.5533430342749538
\]
\[
\frac{1.5533430342749538}{2} \approx 0.7766715171374769
\]
\[
0.7766715171374769 - 0.5 = 0.2766715171374769
\]

### Step 3: Final Answer in JSON Format

\[
\boxed{
\begin{aligned}
\text{"answer": "}\frac{e^{\frac{\pi}{4}} \sqrt{2}}{2} - \frac{1}{2}\text{"}, \\
\text{"numerical_answer": "0.2766715171"}
\end{aligned}
}
\]