Let's start by considering the integral:
\[
I = \int_0^{\pi/4} \frac{\tan(x) + 2\sec^2(x) + 2\tan(x)\sec^2(x)}{\tan(x) + \sec^2(x)}\, dx
\]

**Step 1: Simplify the integrand**

Let’s write the numerator in terms of \(\tan(x)\) and \(\sec^2(x)\):

- Numerator: \(\tan(x) + 2\sec^2(x) + 2\tan(x)\sec^2(x)\)
- Denominator: \(\tan(x) + \sec^2(x)\)

Group \(\tan(x)\) and \(\tan(x)\sec^2(x)\):
\[
\text{Numerator} = \tan(x) + 2\tan(x)\sec^2(x) + 2\sec^2(x)
\]
\[
= \tan(x)[1 + 2\sec^2(x)] + 2\sec^2(x)
\]

But let's try dividing the numerator term by term by the denominator:
Let \(u = \tan(x) + \sec^2(x)\).

Write numerator as:
\[
[\tan(x) + 2\sec^2(x) + 2\tan(x)\sec^2(x)] = [\tan(x) + \sec^2(x)] + [1+\tan(x)]\sec^2(x)
\]
But perhaps better to factor \(\tan(x) + \sec^2(x)\):

Let’s try polynomial (long) division or see if a substitution is useful.

Alternatively, let's let \(u = \tan(x)\). Then \(du = \sec^2(x)\, dx\).

Let’s try that.

When \(x = 0\), \(u = 0\). When \(x = \frac{\pi}{4}\), \(u = 1\).

Let’s convert everything to \(u\):

\[
\tan(x) = u, \quad \sec^2(x) = 1 + u^2, \quad dx = \frac{du}{1 + u^2}
\]

Now substitute:

Numerator:
- \(\tan(x) = u\)
- \(2\sec^2(x) = 2(1 + u^2)\)
- \(2\tan(x)\sec^2(x) = 2u(1 + u^2)\)

Total numerator:
\[
N = u + 2(1 + u^2) + 2u(1 + u^2) = u + 2 + 2u^2 + 2u + 2u^3 = (u + 2u) + 2 + 2u^2 + 2u^3 = 3u + 2 + 2u^2 + 2u^3
\]

Denominator:
\[
D = \tan(x) + \sec^2(x) = u + (1 + u^2) = 1 + u + u^2
\]

Now, the \(dx = du/(1 + u^2)\):

So the whole integrand is, in \(u\):

\[
F(u) = \frac{3u + 2 + 2u^2 + 2u^3}{1 + u + u^2} \cdot \frac{1}{1 + u^2}
\]

Therefore, the entire integral is:

\[
I = \int_{u=0}^{u=1} \frac{3u + 2 + 2u^2 + 2u^3}{(1 + u + u^2)(1 + u^2)} du
\]

**Step 2: Partial Fraction Decomposition**

Let’s decompose

\[
\frac{3u + 2 + 2u^2 + 2u^3}{(1 + u + u^2)(1 + u^2)}
\]

Let’s write numerator in descending order:

\[
2u^3 + 2u^2 + 3u + 2
\]

We seek
\[
\frac{2u^3 + 2u^2 + 3u + 2}{(u^2 + u + 1)(u^2 + 1)} = \frac{Au + B}{u^2 + u + 1} + \frac{Cu + D}{u^2 + 1}
\]

Multiply both sides by \((u^2 + u + 1)(u^2 + 1)\):

\[
2u^3 + 2u^2 + 3u + 2 = (Au + B)(u^2 + 1) + (Cu + D)(u^2 + u + 1)
\]
\[
= Au(u^2 + 1) + B(u^2 + 1) + Cu(u^2 + u + 1) + D(u^2 + u + 1)
\]
\[
= A u^3 + A u + B u^2 + B + C u^3 + C u^2 + C u + D u^2 + D u + D
\]
Group like terms:

- \(u^3\): \(A + C\)
- \(u^2\): \(B + C + D\)
- \(u^1\): \(A + C + D\)
- Constant: \(B + D\)

Wait, let’s actually expand carefully by each term:

\[
(Au + B)(u^2 + 1) = A u^3 + A u + B u^2 + B
\]
\[
(Cu + D)(u^2 + u + 1) = C u^3 + C u^2 + C u + D u^2 + D u + D
\]
So combine:

- \(u^3\): \(A + C\)
- \(u^2\): \(B + C + D\)
- \(u^1\): \(A + C + D\)
- Constant: \(B + D\)

But let's be careful:

Actually, the coefficients from above:
- \(u^3\): \(A + C\)
- \(u^2\): \(B + C + D\)
- \(u^1\): \(A + C + D\)
- Constant: \(B + D\)

Wait: let's expand components explicitly and add for clarity.

1. \(Au \cdot u^2 = Au^3\)
2. \(Au \cdot 1 = Au\)
3. \(B \cdot u^2 = Bu^2\)
4. \(B \cdot 1 = B\)
5. \(Cu \cdot u^2 = Cu^3\)
6. \(Cu \cdot u = Cu^2\)
7. \(Cu \cdot 1 = Cu\)
8. \(D \cdot u^2 = Du^2\)
9. \(D \cdot u = Du\)
10. \(D \cdot 1 = D\)

So sum:

- \(u^3:\) \(Au^3 + Cu^3 = (A + C)u^3\)
- \(u^2:\) \(Bu^2 + Cu^2 + Du^2 = (B + C + D)u^2\)
- \(u^1:\) \(Au + Cu + Du = (A + C + D)u\)
- constants: \(B + D\)

Hence,

\[
2u^3 + 2u^2 + 3u + 2 = (A + C)u^3 + (B + C + D)u^2 + (A + C + D)u + (B + D)
\]

Set equal:

\[
\begin{cases}
A + C = 2 \\
B + C + D = 2 \\
A + C + D = 3 \\
B + D = 2
\end{cases}
\]

Now, solve the system:

First, from \(A + C = 2\) — (1)

 

From \(A + C + D = 3\), so
\[
A + C + D = 3 \implies (A + C) + D = 3 \implies 2 + D = 3 \implies D = 1
\]

From \(B + D = 2\), and \(D = 1\):

\[
B + 1 = 2 \implies B = 1
\]

From \(B + C + D = 2\), so
\[
1 + C + 1 = 2 \implies C = 0
\]

From (1): \(A + 0 = 2 \implies A = 2\)

So,
\[
A = 2,\quad B = 1,\quad C = 0,\quad D = 1
\]

Therefore,

\[
\frac{2u^3 + 2u^2 + 3u + 2}{(u^2 + u + 1)(u^2 + 1)} = \frac{2u + 1}{u^2 + u + 1} + \frac{1}{u^2 + 1}
\]

**Therefore, the integral simplifies to:**

\[
I = \int_0^1 \left[ \frac{2u + 1}{u^2 + u + 1} + \frac{1}{u^2 + 1} \right] du
\]

Let’s split this as \(I = I_1 + I_2\):

\[
I_1 = \int_0^1 \frac{2u + 1}{u^2 + u + 1} du
\]
\[
I_2 = \int_0^1 \frac{1}{u^2 + 1} du
\]

Let's compute \(I_1\):

**Step 3: Compute \(I_1\)**

First, note that \(2u + 1\) is exactly the derivative of the denominator:
\[
\frac{d}{du}(u^2 + u + 1) = 2u + 1
\]
Therefore,
\[
\int \frac{2u + 1}{u^2 + u + 1} du = \ln|u^2 + u + 1| + C
\]

So,
\[
I_1 = \left[ \ln(u^2 + u + 1) \right]_0^1 = \ln(1^2 + 1 + 1) - \ln(0^2 + 0 + 1) = \ln(3) - \ln(1) = \ln 3
\]

**Step 4: Compute \(I_2\)**

\[
I_2 = \int_0^1 \frac{1}{u^2 + 1} du = \arctan(u) \Big|_0^1 = \arctan(1) - \arctan(0) = \frac{\pi}{4} - 0 = \frac{\pi}{4}
\]

**Step 5: Sum up**

\[
I = I_1 + I_2 = \ln 3 + \frac{\pi}{4}
\]

**Step 6: Numerical value**

\[
\ln 3 \approx 1.0986122887
\]
\[
\frac{\pi}{4} \approx 0.7853981634
\]
Therefore,
\[
I \approx 1.0986122887 + 0.7853981634 = 1.8840104521
\]

**Final JSON output:**  
{"answer": "\ln 3 + \\frac{\\pi}{4}", "numerical_answer": "1.8840104521"}