<think>
Okay, let's see. I need to compute the definite integral of sin squared of the natural logarithm of x from 0 to 1. Hmm, that's ∫₀¹ sin²(ln x) dx. Alright, step by step.

First, I remember that sin² terms can sometimes be simplified using a double-angle identity. The identity for sin²θ is (1 - cos(2θ))/2. So maybe I can apply that here. Let me try that substitution.

Let θ = ln x. Then sin²(ln x) becomes (1 - cos(2 ln x))/2. So the integral becomes ∫₀¹ [1 - cos(2 ln x)]/2 dx. That simplifies to (1/2)∫₀¹ 1 dx - (1/2)∫₀¹ cos(2 ln x) dx. The first part is straightforward: (1/2)(1 - 0) = 1/2. But the second integral looks trickier. I need to compute ∫₀¹ cos(2 ln x) dx.

Hmm, how to handle ∫ cos(2 ln x) dx. Maybe substitution? Let me set t = ln x. Then when x is from 0 to 1, t goes from -∞ to 0. So dx = e^t dt. So the integral becomes ∫_{-∞}^0 cos(2t) e^t dt. That's an improper integral from -∞ to 0. Let me check if that's correct. Yes, substitution t = ln x, so x = e^t, dx = e^t dt. So when x approaches 0, t approaches -∞, and x=1 gives t=0. So the integral becomes ∫_{-∞}^0 cos(2t) e^t dt.

Now, I need to compute this integral. Maybe integration by parts? Let me set u = cos(2t), dv = e^t dt. Then du = -2 sin(2t) dt, and v = e^t. So integration by parts gives uv|_{-∞}^0 - ∫ v du. So that's [cos(2t) e^t] from -∞ to 0 minus ∫_{-∞}^0 e^t (-2 sin(2t)) dt. Let's compute the first part. At t=0, cos(0) = 1, e^0 = 1, so term is 1*1 = 1. At t approaching -∞, cos(2t) oscillates, but e^t goes to 0. Since e^t approaches 0 as t→-∞, and cos(2t) is bounded between -1 and 1, the product goes to 0. So the first term is 1 - 0 = 1.

Then the remaining integral is +2 ∫_{-∞}^0 e^t sin(2t) dt. Let's do integration by parts again for this integral. Let u = sin(2t), dv = e^t dt. Then du = 2 cos(2t) dt, v = e^t. So uv|_{-∞}^0 - ∫ v du. The uv term is [sin(2t) e^t] from -∞ to 0. At t=0, sin(0)=0, so that term is 0. At t→-∞, e^t goes to 0, and sin(2t) oscillates but is bounded, so the entire term is 0. So the first part is 0 - 0 = 0. Then the integral becomes - ∫ e^t * 2 cos(2t) dt. So putting it all together, the integral after the first integration by parts is 1 + 2*(0 -2 ∫ e^t cos(2t) dt ). Wait, let me check again.

Wait, after the first integration by parts, we had:

Original integral I = ∫_{-∞}^0 cos(2t) e^t dt = [cos(2t) e^t]_{-∞}^0 + 2 ∫_{-∞}^0 e^t sin(2t) dt = 1 + 2 J, where J = ∫_{-∞}^0 e^t sin(2t) dt.

Then for J, integration by parts gives J = [sin(2t) e^t]_{-∞}^0 - 2 ∫_{-∞}^0 e^t cos(2t) dt = 0 - 2 I. So J = -2 I.

Therefore, substituting back into I: I = 1 + 2*(-2 I) = 1 - 4 I. Then solving for I: I + 4 I = 1 => 5 I = 1 => I = 1/5.

Wait, that seems right. Let me verify. So I = 1 + 2 J, and J = -2 I. Then substituting J into I: I = 1 + 2*(-2 I) = 1 -4 I. Then 5I =1, so I=1/5. Yes, that's correct.

So the integral ∫_{-∞}^0 cos(2t) e^t dt = 1/5. Therefore, going back to the original substitution, the integral of cos(2 ln x) dx from 0 to1 is 1/5. Therefore, the original integral becomes (1/2)(1) - (1/2)(1/5) = (1/2 - 1/10) = (5/10 -1/10)=4/10=2/5. Wait, that's 0.4. But let me check again.

Wait, the original integral was ∫₀¹ sin²(ln x) dx = (1/2)∫₀¹ 1 dx - (1/2)∫₀¹ cos(2 ln x) dx. The first integral is 1/2 *1 =1/2. The second integral is (1/2)*(1/5)=1/10. So 1/2 -1/10= (5-1)/10=4/10=2/5. So the exact answer is 2/5. Hmm, but let me check if that's correct.

Wait, but when I did the substitution for the integral of cos(2 ln x) dx, I got 1/5. So yes, (1/2)(1 -1/5)= (1/2)(4/5)=2/5. So the exact answer is 2/5. But wait, let me check with another method to be sure.

Alternatively, maybe use substitution in the original integral. Let me set t = ln x. Then x = e^t, dx = e^t dt. When x=0, t approaches -infty; x=1, t=0. So the integral becomes ∫_{-infty}^0 sin²(t) e^t dt. Then using the same identity, sin² t = (1 - cos(2t))/2. So the integral becomes ∫_{-infty}^0 [1 - cos(2t)]/2 * e^t dt = (1/2)∫ e^t dt - (1/2)∫ cos(2t) e^t dt. The first integral is (1/2)[e^t]_{-infty}^0 = (1/2)(1 -0)=1/2. The second integral is (1/2) * (1/5) as before, so total is 1/2 -1/10=2/5. So same result. So that's correct.

Therefore, the exact answer is 2/5. Then the numerical approximation. 2 divided by 5 is 0.4. But let me check if there's any mistake here. Wait, 2/5 is 0.4 exactly. So the numerical approximation is 0.4. But wait, is that correct? Let me check with a numerical integration.

Wait, maybe I made a mistake in the integral. Let me compute ∫₀¹ sin²(ln x) dx numerically. Let's approximate it. For example, using substitution x = e^{-y}, so when x=0, y approaches infinity, x=1, y=0. Then dx = -e^{-y} dy. The integral becomes ∫_{0}^{infty} sin²(-y) e^{-y} dy. Since sin(-y) = -sin y, so sin²(-y)=sin² y. So the integral is ∫₀^infty sin² y e^{-y} dy. Then sin² y = (1 - cos(2y))/2. So integral becomes (1/2)∫₀^infty e^{-y} dy - (1/2)∫₀^infty cos(2y) e^{-y} dy. The first integral is (1/2)(1) =1/2. The second integral can be evaluated using the formula ∫₀^infty e^{-a y} cos(b y) dy = a/(a² + b²). Here, a=1, b=2. So the integral is 1/(1² +2²)=1/5. So the second term is (1/2)*(1/5)=1/10. So total integral is 1/2 -1/10=2/5=0.4. So yes, the numerical value is exactly 0.4, so 0.4000000000 when rounded to 10 decimal places.

Therefore, the exact answer is 2/5, and the numerical is 0.4. So the JSON should be {"answer": "\\dfrac{2}{5}", "numerical_answer": 0.4000000000}.
</think>

{"answer": "\\dfrac{2}{5}", "numerical_answer": 0.4000000000}