Let's solve the integral
\[
I = \int_0^\pi \cos(x+\cos x) \; dx
\]

**Step 1: Analytical Computation**

Let us use a substitution. Let
\[
u = x + \cos x \implies du = (1 - \sin x)\,dx
\]
But this is awkward. Let's try integrating by parts:
Let \( u = \sin(x+\cos x) \), \( dv = dx \):

Let’s instead try writing
\[
\cos(x+\cos x) = \Re\left( e^{i(x+\cos x)} \right)
\]
Let’s expand:
\[
e^{i(x+\cos x)} = e^{ix} e^{i\cos x}
\]
But this does not immediately help.

Let us use the substitution symmetry \( x \mapsto \pi - x \):

Let \( J = \int_0^\pi \cos(x+\cos x)dx \)

Substitute \( y = \pi - x \Rightarrow x = \pi - y, \ dx = -dy \); as \( x \) goes from 0 to \( \pi \), \( y \) goes from \( \pi \) to 0.

\[
J = \int_0^\pi \cos(x + \cos x) dx = \int_{\pi}^0 \cos(\pi - y + \cos(\pi - y)) \cdot (-dy)
\]
\[
= \int_0^\pi \cos(\pi - y + \cos(\pi - y)) dy
\]
But \(\cos(\pi - y) = -\cos y\), so
\[
\cos(\pi - y + \cos(\pi - y)) = \cos(\pi - y - \cos y)
\]
But \(\cos(A + B) = \cos A \cos B - \sin A \sin B\).

But we have:
\[
J = \int_0^\pi \cos(\pi - x - \cos x) dx = \int_0^\pi \cos[ \pi - (x + \cos x) ] dx
\]
And \(\cos[\pi - \theta] = -\cos \theta\), so
\[
J = \int_0^\pi - \cos( x + \cos x ) dx = - J
\]
So,
\[
J = -J \implies J = 0
\]
Therefore,

\[
\boxed{ \int_0^{\pi} \cos(x+\cos x)\, dx = 0 }
\]

**Step 2: Steps Shown Above**

- Substituted \(x \mapsto \pi - x\), which transforms the integral into its negative.
- Concluded the value must be zero.

**Step 3: Numerical Approximation**

Clearly, the answer is exactly 0. For completeness, the numerical value is
\[
0.0000000000
\]

**JSON Output:**
```json
{"answer": "0", "numerical_answer": "0.0000000000"}
```