To solve
  I = ∫₀^(π/4) [tan(x) + 2 sec²(x) + 2 tan(x) sec²(x)] / [tan(x) + sec²(x)] dx,
we first try to recognize a derivative structure in the integrand.

Step 1. Write the denominator as
  u(x) = tan(x) + sec²(x).

Differentiate u(x) with respect to x:
  u'(x) = sec²(x) + 2 sec²(x) tan(x)
      = sec²(x) (1 + 2 tan(x)).

Step 2. Notice that if we differentiate the function
  F(x) = x + ln(u(x)) = x + ln(tan(x) + sec²(x)),
its derivative is
  F'(x) = 1 + u'(x)/u(x) = 1 + [sec²(x)(1 + 2 tan(x))] / [tan(x) + sec²(x)].

Combine the terms over the common denominator:
  1 = (tan(x) + sec²(x))/(tan(x) + sec²(x)),
so
  F'(x) = [tan(x) + sec²(x) + sec²(x) (1 + 2 tan(x))] / [tan(x) + sec²(x)].
Simplify the numerator:
  tan(x) + sec²(x) + sec²(x) + 2 tan(x) sec²(x)
   = tan(x) + 2 sec²(x) + 2 tan(x) sec²(x).

Thus, we have
  F'(x) = [tan(x) + 2 sec²(x) + 2 tan(x) sec²(x)] / [tan(x) + sec²(x)],
which is exactly our given integrand.

Step 3. Hence, the antiderivative is
  F(x) = x + ln(tan(x) + sec²(x)).

Now, evaluate from 0 to π/4:
At x = π/4:
  tan(π/4) = 1, sec²(π/4) = 2,
so
  F(π/4) = (π/4) + ln(1 + 2) = (π/4) + ln(3).

At x = 0:
  tan(0) = 0, sec²(0) = 1,
so
  F(0) = 0 + ln(0 + 1) = ln(1) = 0.

Thus, the value of the integral is:
  I = F(π/4) – F(0) = (π/4) + ln(3).

Step 4. Numerical approximation:
  π/4 ≈ 0.7853981634,
  ln(3) ≈ 1.0986122887,
so the sum is approximately 0.7853981634 + 1.0986122887 ≈ 1.8840104521.

The final answer is provided below in the required JSON format.

{"answer": "\\frac{\\pi}{4}+\\ln(3)", "numerical_answer": "1.8840104521"}