Let's denote the integral as
\[
I = \int_{-e}^e \frac{e^{-x^{2024}}\cos(2024x)}{\arctan(2024x)}\,dx.
\]

**Step 1: Analyze the integrand's symmetry.**

Let
\[
f(x) = \frac{e^{-x^{2024}}\cos(2024x)}{\arctan(2024x)}.
\]

Consider \( f(-x) \):
\[
f(-x) = \frac{e^{-(-x)^{2024}}\cos(2024 \cdot -x)}{\arctan(2024 \cdot -x)}
= \frac{e^{-x^{2024}}\cos(-2024x)}{\arctan(-2024x)}.
\]
Since cosine is even, \( \cos(-2024x) = \cos(2024x) \). And,
\[
\arctan(-2024x) = -\arctan(2024x).
\]

Therefore,
\[
f(-x) = \frac{e^{-x^{2024}}\cos(2024x)}{-\arctan(2024x)} = -f(x).
\]
So \( f(x) \) is an **odd function**.

**Step 2: Use the odd function property over symmetric interval.**

Since \( f(x) \) is odd and the limits are symmetric about \( 0 \):
\[
I = \int_{-e}^e f(x)\,dx = 0.
\]

**Step 3: Numerical evaluation**

Zero is the numerical result.

**Step 4: Output in required JSON format**

```json
{"answer": "0", "numerical_answer": "0.0000000000"}
```