We wish to evaluate

  I = ∫₀⁷ (³√(√(x²+1)+x) − ³√(√(x²+1)−x)) dx.

Step 1. Rewrite the integrand

Define
  A = ³√(√(x²+1)+x)  and  B = ³√(√(x²+1)−x).

Then we have
  A³ = √(x²+1)+x  and  B³ = √(x²+1)−x.
Notice that multiplying A³ and B³:
  A³ B³ = (√(x²+1)+x)(√(x²+1)−x) = (x²+1) - x² = 1.
Thus,
  A · B = ¹³√(1) = 1  or  B = 1/A.

Now, the integrand becomes
  f(x) = A − B = A − 1/A.

Step 2. An algebraic trick

Set y = f(x) = A − 1/A. Notice that
  (A − 1/A)³ = A³ − 3A (1/A)(A − 1/A) − 1/A³
because by the cube formula:
  (A − 1/A)³ = A³ − 3A(1/A)(A − 1/A) + (1/A)³ (with a sign change since (−1/A)³ = −1/A³).
Thus,
  (A − 1/A)³ = A³ − 1/A³ − 3(A − 1/A).

But recall A³ and B³ and that 1/A³ = B³. So
  A³ − 1/A³ = (√(x²+1)+x) − (√(x²+1)−x) = 2x.
It follows that
  y³ = 2x − 3y  or  y³ + 3y = 2x.
Thus, we can express x in terms of y:
  x = (y³ + 3y)/2.            (1)

Step 3. Changing variables in the integral

Since we want to rewrite the integral in terms of y, differentiate equation (1):

  dx/dy = d/dy[(y³+3y)/2] = (3y²+3)/2 = (3(y²+1))/2.
Hence, dx = (3(y²+1)/2) dy.

Also, note that our integrand f(x) is exactly y. So when substituting,
  I = ∫ (f(x) dx) becomes
  I = ∫ y · dx = ∫ y · (3(y²+1)/2) dy = (3/2) ∫ y(y²+1) dy.

Step 4. Determine the new limits

When x = 0, substitute in equation (1):
  0 = (y³+3y)/2  ⟹  y(y²+3)=0  ⟹  y = 0.
When x = 7,
  7 = (y³+3y)/2  ⟹  y³+3y = 14.
Test y = 2:
  2³ + 3·2 = 8 + 6 = 14.
Thus, when x=7, y=2.

Step 5. Evaluate the new integral

Our integral is now
  I = (3/2) ∫₀² y(y²+1) dy.
Expand the integrand:
  y(y²+1) = y³ + y.
Thus,
  I = (3/2) ∫₀² (y³ + y) dy.

Compute the antiderivative:
  ∫ (y³+y) dy = y⁴/4 + y²/2.
Evaluate from 0 to 2:
  At y=2: (16/4)+(4/2)= 4+2 = 6.
  At y=0: 0.
Thus,
  I = (3/2) · 6 = 9.

Step 6. Summary of results

The exact value of the integral is 9. Numerically, 9 = 9.0000000000 (when rounded to 10 decimal places).

Final Answer in JSON format:
{"answer": "$9$", "numerical_answer": "$9.0000000000$"}