Let's solve the integral step by step:

\[
I = \int_0^{\pi/4} \frac{\tan(x) + 2\sec^2(x) + 2\tan(x)\sec^2(x)}{\tan(x) + \sec^2(x)} \, dx
\]

### Step 1: Simplify the Integrand
First, observe the denominator and numerator:

Denominator: \( \tan(x) + \sec^2(x) \)

Numerator: \( \tan(x) + 2\sec^2(x) + 2\tan(x)\sec^2(x) \)

Notice that the numerator can be rewritten as:
\[
\tan(x) + 2\sec^2(x) + 2\tan(x)\sec^2(x) = (\tan(x) + \sec^2(x)) + \sec^2(x) + 2\tan(x)\sec^2(x)
\]

But this doesn't immediately simplify. Instead, let's consider a substitution.

### Step 2: Substitution
Let \( u = \tan(x) + \sec^2(x) \).

Compute \( du \):
\[
\sec^2(x) = 1 + \tan^2(x) \implies u = \tan(x) + 1 + \tan^2(x) = \tan^2(x) + \tan(x) + 1
\]
\[
du = (2\tan(x) + 1)\sec^2(x) \, dx
\]

Now, look at the numerator:
\[
\tan(x) + 2\sec^2(x) + 2\tan(x)\sec^2(x) = (\tan(x) + \sec^2(x)) + \sec^2(x) + 2\tan(x)\sec^2(x)
\]
\[
= u + \sec^2(x) + 2\tan(x)\sec^2(x)
\]

This still doesn't directly match \( du \), but let's express everything in terms of \( u \):

From \( u = \tan^2(x) + \tan(x) + 1 \), we can solve for \( \tan(x) \), but this seems complicated. Instead, let's try another approach.

### Step 3: Rewrite the Integrand
Divide the numerator by the denominator:
\[
\frac{\tan(x) + 2\sec^2(x) + 2\tan(x)\sec^2(x)}{\tan(x) + \sec^2(x)} = 1 + \frac{\sec^2(x) + 2\tan(x)\sec^2(x)}{\tan(x) + \sec^2(x)}
\]
\[
= 1 + \frac{\sec^2(x)(1 + 2\tan(x))}{\tan(x) + \sec^2(x)}
\]

Now, notice that:
\[
\frac{d}{dx}[\tan(x) + \sec^2(x)] = \sec^2(x) + 2\sec^2(x)\tan(x) = \sec^2(x)(1 + 2\tan(x))
\]

This is exactly the numerator of the second term! So, the integrand simplifies to:
\[
1 + \frac{u'}{u}
\]
where \( u = \tan(x) + \sec^2(x) \).

Thus:
\[
I = \int_0^{\pi/4} \left(1 + \frac{u'}{u}\right) dx = \int_0^{\pi/4} 1 \, dx + \int_0^{\pi/4} \frac{u'}{u} \, dx
\]
\[
= \left. x \right|_0^{\pi/4} + \left. \ln|u| \right|_0^{\pi/4}
\]

### Step 4: Evaluate the Integrals
Compute \( u \) at the bounds:
At \( x = \pi/4 \):
\[
\tan(\pi/4) = 1, \quad \sec^2(\pi/4) = 2 \implies u = 1 + 2 = 3
\]

At \( x = 0 \):
\[
\tan(0) = 0, \quad \sec^2(0) = 1 \implies u = 0 + 1 = 1
\]

Now, evaluate the integrals:
\[
I = \left( \frac{\pi}{4} - 0 \right) + \left( \ln(3) - \ln(1) \right) = \frac{\pi}{4} + \ln(3)
\]

### Step 5: Numerical Approximation
Compute the numerical value:
\[
\frac{\pi}{4} \approx 0.7853981634
\]
\[
\ln(3) \approx 1.0986122887
\]
\[
I \approx 0.7853981634 + 1.0986122887 = 1.8840104521
\]

### Final Answer
\[
\boxed{
{"answer": "\frac{\pi}{4} + \ln(3)", "numerical_answer": "1.8840104521"}
}
\]