# Evaluating $\int_0^{\frac{\pi}{2}}\frac{\ln(\sin x)}{\cos^2x}\mathrm{d}x$

## Step 1: Substitution
Let's start with the substitution $u = \sin x$. This gives us:
- $\cos x \, dx = du$
- When $x = 0$, $u = 0$
- When $x = \frac{\pi}{2}$, $u = 1$

For our integral:
$\frac{\ln(\sin x)}{\cos^2x}\mathrm{d}x = \frac{\ln(u)}{\cos x} \cdot \frac{du}{\cos x} = \frac{\ln(u)}{\cos^2 x}dx$

Since $\cos^2 x = 1 - \sin^2 x = 1 - u^2$, we get:
$\int_0^{\frac{\pi}{2}}\frac{\ln(\sin x)}{\cos^2x}\mathrm{d}x = \int_0^{1}\frac{\ln(u)}{1-u^2}du$

## Step 2: Partial fractions decomposition
We can write:
$\frac{1}{1-u^2} = \frac{1}{(1-u)(1+u)} = \frac{1/2}{1-u} + \frac{1/2}{1+u}$

So our integral becomes:
$\int_0^{1}\frac{\ln(u)}{1-u^2}du = \frac{1}{2}\int_0^{1}\frac{\ln(u)}{1-u}du + \frac{1}{2}\int_0^{1}\frac{\ln(u)}{1+u}du$

## Step 3: Evaluate the first part
For $\int_0^{1}\frac{\ln(u)}{1-u}du$, let's use the substitution $v = 1-u$:
- When $u = 0$, $v = 1$
- When $u = 1$, $v = 0$
- $du = -dv$
- $\ln(u) = \ln(1-v)$

This gives us:
$\int_0^{1}\frac{\ln(u)}{1-u}du = -\int_1^{0}\frac{\ln(1-v)}{v}dv = \int_0^{1}\frac{\ln(1-v)}{v}dv$

This is a known integral form that evaluates to $-\frac{\pi^2}{6}$. This is the dilogarithm function $\text{Li}_2(1) = \frac{\pi^2}{6}$, but with a negative sign due to the logarithm term.

## Step 4: Evaluate the second part
For $\int_0^{1}\frac{\ln(u)}{1+u}du$, we can use integration by parts:
Let $p = \ln(u)$ and $dq = \frac{1}{1+u}du$

Then $dp = \frac{1}{u}du$ and $q = \ln(1+u)$

$\int_0^{1}\frac{\ln(u)}{1+u}du = \ln(u)\ln(1+u)\Big|_0^{1} - \int_0^{1}\frac{\ln(1+u)}{u}du$

The first term evaluates to $\ln(1)\ln(2) - \ln(0)\ln(1) = 0 - (-\infty) \cdot 0$. The $\ln(0)$ term introduces an apparent singularity, but the product $\ln(0)\ln(1)$ equals 0 in the limit as $u$ approaches 0.

The second term is $-\int_0^{1}\frac{\ln(1+u)}{u}du = -\text{Li}_2(1) = -\frac{\pi^2}{6}$

Therefore, $\int_0^{1}\frac{\ln(u)}{1+u}du = -\frac{\pi^2}{6}$

## Step 5: Combine the results
Now we can combine our results:
$\int_0^{\frac{\pi}{2}}\frac{\ln(\sin x)}{\cos^2x}\mathrm{d}x = \frac{1}{2} \cdot (-\frac{\pi^2}{6}) + \frac{1}{2} \cdot (-\frac{\pi^2}{6}) = -\frac{\pi^2}{6}$

## Numerical Approximation
$-\frac{\pi^2}{6} \approx -1.6449340668$ (rounded to 10 decimal places)

{"answer": "-\\frac{\\pi^2}{6}", "numerical_answer": "-1.6449340668"}