Let's tackle the integral:
\[
I = \int_{0}^{2} H_3\left(\sqrt{x(2-x)}\right) dx
\]
where \( H_3(x) \) is the third Hermite polynomial.

**Step 1: Hermite polynomial identification**

The third Hermite polynomial is:
\[
H_3(x) = 8x^3 - 12x
\]

**Step 2: Substitute \( x \to \sqrt{x(2-x)} \) into \( H_3 \):**

So,
\[
H_3\left(\sqrt{x(2-x)}\right) = 8 \left(\sqrt{x(2-x)}\right)^3 - 12 \left(\sqrt{x(2-x)}\right)
\]
\[
= 8 \left(x(2-x)\right)^{3/2} - 12 \left(x(2-x)\right)^{1/2}
\]

So the integral becomes:
\[
I = \int_{0}^{2} \left[8(x(2-x))^{3/2} - 12(x(2-x))^{1/2}\right] dx
\]
\[
= 8 \int_{0}^{2} (x(2-x))^{3/2} dx - 12 \int_{0}^{2} (x(2-x))^{1/2} dx
\]

Let us denote:
\[
I_1 = \int_{0}^{2} (x(2-x))^{3/2} dx;\qquad I_2 = \int_{0}^{2} (x(2-x))^{1/2} dx
\]
So
\[
I = 8 I_1 - 12 I_2
\]

**Step 3: Solve each integral with substitution**

Note:
\[
x(2-x) = 2x - x^2
\]

Let’s use the substitution \( x = 2\sin^2\theta \), so that as \( x \) goes from 0 to 2, \(\theta\) goes from 0 to \(\pi/2\):

- When \( x = 0 \), \(\sin \theta = 0 \implies \theta = 0\)
- When \( x = 2 \), \(2\sin^2\theta = 2 \implies \sin^2\theta = 1 \implies \theta = \pi/2\)

Now, compute:
\[
x = 2\sin^2\theta \implies dx = 4\sin\theta\cos\theta d\theta = 2\sin 2\theta d\theta
\]
\[
x(2-x) = 2\sin^2\theta (2 - 2\sin^2\theta) = 4\sin^2\theta \cos^2\theta = (\sin 2\theta)^2
\]

Thus,
- \((x(2-x))^{1/2} = |\sin 2\theta|\) (but \(0 \leq \theta \leq \pi/2\) so positive).
- \((x(2-x))^{3/2} = (\sin 2\theta)^3\)

Let’s rewrite:
\[
I_1 = \int_{0}^{2} (x(2-x))^{3/2} dx = \int_{\theta=0}^{\pi/2} (\sin 2\theta)^3 \cdot 2\sin 2\theta d\theta
= 2 \int_{0}^{\pi/2} (\sin 2\theta)^4 d\theta
\]

Similarly:
\[
I_2 = \int_{0}^{2} (x(2-x))^{1/2} dx = \int_{0}^{\pi/2} \sin 2\theta \cdot 2\sin 2\theta d\theta
= 2 \int_{0}^{\pi/2} (\sin 2\theta)^2 d\theta
\]

**So:**
\[
I = 8I_1 - 12I_2 = 8 \cdot 2\int_{0}^{\pi/2} (\sin 2\theta)^4 d\theta - 12 \cdot 2 \int_{0}^{\pi/2} (\sin 2\theta)^2 d\theta
= 16 \int_{0}^{\pi/2} (\sin 2\theta)^4 d\theta - 24 \int_{0}^{\pi/2} (\sin 2\theta)^2 d\theta
\]

Let’s let
\[
J_1 = \int_{0}^{\pi/2} (\sin 2\theta)^4 d\theta
\]
\[
J_2 = \int_{0}^{\pi/2} (\sin 2\theta)^2 d\theta
\]

So:
\[
I = 16 J_1 - 24 J_2
\]

---

**Step 4: Compute \( J_1 \) and \( J_2 \) analytically**

**(A) \( J_2 = \int_0^{\pi/2} (\sin 2\theta)^2 d\theta \)**
\[
(\sin 2\theta)^2 = \frac{1}{2} (1 - \cos 4\theta)
\]
So,
\[
J_2 = \int_0^{\pi/2} \frac{1}{2} (1 - \cos 4\theta) d\theta = \frac{1}{2} \int_0^{\pi/2} d\theta - \frac{1}{2} \int_0^{\pi/2} \cos 4\theta d\theta
\]
\[
= \frac{1}{2} \cdot \frac{\pi}{2} - \frac{1}{2} \left[ \frac{\sin 4\theta}{4} \Big|_{0}^{\pi/2} \right]
\]
\[
\sin(4\cdot \pi/2) = \sin 2\pi = 0
\]
\[
\sin(0) = 0
\]
\[
J_2 = \frac{\pi}{4} - \frac{1}{2} \cdot 0 = \frac{\pi}{4}
\]

**(B) \( J_1 = \int_0^{\pi/2} (\sin 2\theta)^4 d\theta \)**
\[
(\sin 2\theta)^4 = [\sin^2 2\theta]^2 = \left( \frac{1 - \cos 4\theta}{2} \right)^2 = \frac{1}{4}(1 - 2\cos 4\theta + \cos^2 4\theta)
\]
But,
\[
\cos^2 4\theta = \frac{1 + \cos 8\theta}{2}
\]
So,
\[
(\sin 2\theta)^4 = \frac{1}{4} \left(1 - 2\cos 4\theta + \frac{1 + \cos 8\theta}{2}\right)
= \frac{1}{4}\left(1 - 2\cos 4\theta + \frac{1}{2} + \frac{1}{2} \cos 8\theta\right)
= \frac{1}{4}\left(\frac{3}{2} - 2\cos 4\theta + \frac{1}{2} \cos 8\theta\right)
\]
\[
= \frac{3}{8} - \frac{1}{2}\cos 4\theta + \frac{1}{8}\cos 8\theta
\]

Therefore,
\[
J_1 = \int_0^{\pi/2} \left(\frac{3}{8} - \frac{1}{2}\cos 4\theta + \frac{1}{8}\cos 8\theta\right) d\theta
= \frac{3}{8} \int_0^{\pi/2} d\theta - \frac{1}{2} \int_0^{\pi/2} \cos 4\theta d\theta + \frac{1}{8} \int_0^{\pi/2} \cos 8\theta d\theta
\]

The three integrals are:
- \(\int_0^{\pi/2} d\theta = \frac{\pi}{2}\)
- \(\int_0^{\pi/2} \cos 4\theta d\theta = \frac{1}{4} [\sin 4\theta]_0^{\pi/2} = \frac{1}{4}(\sin 2\pi - \sin 0) = 0\)
- \(\int_0^{\pi/2} \cos 8\theta d\theta = \frac{1}{8} [\sin 8\theta]_0^{\pi/2} = \frac{1}{8} (\sin 4\pi - \sin 0) = 0\)

So,
\[
J_1 = \frac{3}{8} \cdot \frac{\pi}{2} - 0 + 0 = \frac{3\pi}{16}
\]

---

**Step 5: Substitute results**
\[
I = 16 J_1 - 24 J_2 = 16 \cdot \frac{3\pi}{16} - 24 \cdot \frac{\pi}{4} = 3\pi - 6\pi = -3\pi
\]

---

**Step 6: Numerical value**
\[
-3\pi \approx -3 \times 3.1415926536 = -9.4247779608
\]

---

**Final Answers:**
- Exact: \( -3\pi \)
- Numerical (rounded to 10 decimal places): \( -9.4247779608 \)

---

```json
{"answer": "-3\\pi", "numerical_answer": "-9.4247779608"}
```