We wish to compute

  I = ∫₀^(π/4) arctan[(1 + tan x)/√2] dx.

Step 1. A Helpful Change of Variable

A useful trick is to use the substitution
  u = (π/4) − x.
Then
  dx = −du,
and when x = 0, u = π/4; when x = π/4, u = 0. Changing the limits we have

  I = ∫₀^(π/4) arctan[(1 + tan x)/√2] dx
    = ∫_(u=π/4)^(0) arctan[(1 + tan(π/4 − u))/√2] (−du)
    = ∫₀^(π/4) arctan[(1 + tan(π/4 − u))/√2] du.

Now use the tangent subtraction formula:
  tan(π/4 − u) = (tan(π/4) − tan u)/(1 + tan(π/4)tan u)
         = (1 − tan u)/(1 + tan u).

Thus inside the arctan we have:
  (1 + tan(π/4 − u))/√2
    = [1 + ((1 − tan u)/(1 + tan u))] / √2
    = [( (1 + tan u) + (1 − tan u) )/(1 + tan u)] / √2
    = [2/(1 + tan u)]/√2
    = √2/(1 + tan u).

Thus the integral becomes
  I = ∫₀^(π/4) arctan[√2/(1 + tan u)] du.

Since u is a dummy variable, we rename it back to x and denote the new integral as:
  I = ∫₀^(π/4) arctan[√2/(1 + tan x)] dx.

Step 2. Adding Two Representations

Now denote the original integral by I₁:
  I₁ = ∫₀^(π/4) arctan[(1 + tan x)/√2] dx,
and the transformed one by I₂:
  I₂ = ∫₀^(π/4) arctan[√2/(1 + tan x)] dx.

Notice that for any positive number a,
  arctan a + arctan(1/a) = π/2.
Here, let
  a = (1 + tan x)/√2  (positive for x in [0, π/4]).
Then,
  arctan[(1 + tan x)/√2] + arctan[√2/(1 + tan x)] = π/2.

Thus adding I₁ and I₂ we get:
  I₁ + I₂ = ∫₀^(π/4) [arctan((1 + tan x)/√2) + arctan(√2/(1 + tan x))] dx
        = ∫₀^(π/4) (π/2) dx
        = (π/2)·(π/4) = π²/8.

Since we have shown that I₁ = I₂ = I, it follows that
  2I = π²/8  ⟹  I = π²/16.

Step 3. Numerical Approximation

We have
  π²/16 = (approximately 9.869604401089358)/(16) ≈ 0.6168502751.

Final Answer in JSON format:

{"answer": "\\frac{\\pi^2}{16}", "numerical_answer": "0.6168502751"}