<think>
Okay, let's see. I need to compute the definite integral from 0 to 4 of x^(-1/2)(4 - x)^(-1/2)[1 - 0.25x(4 - x)]^(1/2) dx. Hmm, that looks a bit complicated, but maybe there's a substitution or a known integral form that can help here.

First, let me rewrite the integrand to make it clearer. The integrand is x^{-1/2} (4 - x)^{-1/2} [1 - 0.25x(4 - x)]^{1/2}. Let me simplify the expression inside the square root first. The term 0.25x(4 - x) can be expanded. Let's compute that:

0.25x(4 - x) = 0.25*(4x - x²) = x - 0.25x². So, 1 - 0.25x(4 - x) = 1 - x + 0.25x². Wait, that's a quadratic in x. Let me check that again.

Wait, 0.25x(4 - x) is 0.25*4x - 0.25x² = x - 0.25x². So 1 - (x - 0.25x²) = 1 - x + 0.25x². Let me see if that quadratic can be written as a square. Let's see:

1 - x + 0.25x². Let's arrange the terms: 0.25x² - x + 1. Let's factor out 0.25 from the first two terms: 0.25(x² - 4x) + 1. Completing the square inside the parentheses: x² - 4x + 4 - 4 = (x - 2)^2 - 4. So, 0.25[(x - 2)^2 - 4] + 1 = 0.25(x - 2)^2 - 1 + 1 = 0.25(x - 2)^2. Wait, that can't be right. Let me check again.

Wait, 0.25x² - x + 1. Let me write it as (0.5x)^2 - x + 1. Hmm, maybe another approach. Let's check if 0.25x² - x + 1 is a perfect square. Suppose it's (ax + b)^2. Then, a²x² + 2abx + b². Comparing coefficients:

a² = 0.25 => a = 0.5 or -0.5

2ab = -1. Let's take a = 0.5. Then 2*0.5*b = -1 => b = -1. Then, (0.5x - 1)^2 = 0.25x² - x + 1. Yes! So, 1 - x + 0.25x² = (0.5x - 1)^2. Therefore, the square root of that is |0.5x - 1|. But since we're integrating from 0 to 4, let's see the sign of 0.5x - 1 in that interval.

At x=0: 0 - 1 = -1, so 0.5*0 -1 = -1. At x=4: 0.5*4 -1 = 2 -1 = 1. So, the expression inside the square root is (0.5x -1)^2, so the square root is |0.5x -1|. Therefore, the integrand becomes x^{-1/2}(4 - x)^{-1/2} |0.5x -1|.

But since the integral is from 0 to 4, let's split it at x=2 where 0.5x -1 changes sign. So, from 0 to 2, 0.5x -1 is negative, so |0.5x -1| = 1 - 0.5x. From 2 to 4, it's positive, so |0.5x -1| = 0.5x -1. Therefore, the integral becomes the sum of two integrals:

Integral from 0 to 2 of x^{-1/2}(4 - x)^{-1/2}(1 - 0.5x) dx + Integral from 2 to 4 of x^{-1/2}(4 - x)^{-1/2}(0.5x -1) dx.

Hmm, but maybe there's a substitution that can handle this without splitting. Alternatively, perhaps a beta function or gamma function is involved here. Let me recall that the integral from 0 to 1 of t^{a-1}(1 - t)^{b-1} dt is the Beta function B(a, b) = Γ(a)Γ(b)/Γ(a + b). But our integral is from 0 to 4, but maybe a substitution can transform it into a Beta function.

Alternatively, let's make a substitution to simplify the limits. Let me set t = x/4, so x = 4t, dx = 4dt. Then, when x=0, t=0; x=4, t=1. Then, the integral becomes:

Integral from t=0 to t=1 of (4t)^{-1/2}(4 - 4t)^{-1/2}[1 - 0.25*(4t)(4 - 4t)]^{1/2} *4 dt.

Simplify each term:

(4t)^{-1/2} = (4)^{-1/2} t^{-1/2} = (1/2) t^{-1/2}

(4 - 4t)^{-1/2} = (4(1 - t))^{-1/2} = (1/2)(1 - t)^{-1/2}

The term inside the square root: 1 - 0.25*(4t)(4 - 4t) = 1 - 0.25*16t(1 - t) = 1 - 4t(1 - t) = 1 - 4t(1 - t). Wait, 0.25*4t*(4 -4t) = 0.25*4t*4(1 - t) = 4t(1 - t). So, 1 - 4t(1 - t). Hmm, that's 1 -4t +4t². Which is (2t -1)^2. Because (2t -1)^2 = 4t² -4t +1. So, 1 -4t(1 -t) = 1 -4t +4t² = (2t -1)^2. Therefore, the square root of that is |2t -1|. So, the integrand becomes:

(1/2 t^{-1/2}) * (1/2 (1 - t)^{-1/2}) * |2t -1| *4 dt.

Multiply the constants: (1/2)(1/2)*4 = 1. So, the integral becomes:

∫₀¹ t^{-1/2}(1 - t)^{-1/2} |2t -1| dt.

Now, split the integral at t=1/2 where 2t -1 changes sign. So:

Integral from 0 to 1/2 of t^{-1/2}(1 - t)^{-1/2}(1 - 2t) dt + Integral from 1/2 to 1 of t^{-1/2}(1 - t)^{-1/2}(2t -1) dt.

Hmm, but maybe there's a better way. Let's consider substitution. Let me see if the integral can be expressed in terms of Beta functions with some linear terms. Alternatively, perhaps using substitution u = t(1 - t) or something else. Alternatively, note that t^{-1/2}(1 - t)^{-1/2} is the integrand of the Beta function B(1/2, 1/2) which is π. But here we have an extra factor of |2t -1|. So, perhaps we can compute this integral by expanding or using known integrals.

Alternatively, consider substitution u = 2t -1. Let's try that. Let u = 2t -1. Then, when t=0, u=-1; t=1, u=1; t=1/2, u=0. Then, dt = du/2. The integral becomes:

∫_{-1}^1 [ ( (u +1)/2 )^{-1/2} (1 - (u +1)/2 )^{-1/2} |u| ] * (du/2)

Simplify the terms inside the brackets:

First term: ( (u +1)/2 )^{-1/2} = [ (u +1)/2 ]^{-1/2} = (2/(u +1))^{1/2}

Second term: (1 - (u +1)/2 )^{-1/2} = ( (2 - u -1)/2 )^{-1/2} = ( (1 - u)/2 )^{-1/2} = (2/(1 - u))^{1/2}

So, multiplying these two terms: (2/(u +1))^{1/2} * (2/(1 - u))^{1/2} = (4 / [(1 + u)(1 - u)])^{1/2} = (4 / (1 - u²))^{1/2} = 2 / sqrt(1 - u²)

Therefore, the integral becomes:

∫_{-1}^1 [2 / sqrt(1 - u²)] * |u| * (du/2) = ∫_{-1}^1 |u| / sqrt(1 - u²) du

Since the integrand is even (|u| is even, sqrt(1 - u²) is even), we can compute 2 times the integral from 0 to 1:

2 * ∫₀¹ u / sqrt(1 - u²) du

Let me compute this integral. Let’s set v = 1 - u², dv = -2u du, so -dv/2 = u du. Then, when u=0, v=1; u=1, v=0. So, the integral becomes:

2 * ∫₁⁰ (sqrt(v))^{-1} * (-dv/2) ) = 2 * (1/2) ∫₀¹ v^{-1/2} dv = ∫₀¹ v^{-1/2} dv = [2 v^{1/2}]₀¹ = 2(1 - 0) = 2.

Wait, so the integral ∫_{-1}^1 |u| / sqrt(1 - u²) du = 2. Therefore, the original integral after substitution is 2. But wait, let's check the steps again.

Wait, after substitution, the integral became ∫_{-1}^1 |u| / sqrt(1 - u²) du, which is 2. So, the original integral from 0 to 4 is equal to 2? But let's check the steps again to make sure.

Original integral after substitution t = x/4 became ∫₀¹ t^{-1/2}(1 - t)^{-1/2} |2t -1| dt. Then substitution u = 2t -1 led to the integral being 2. So, the original integral is 2. But let me verify with a numerical approximation. Let's compute the numerical value. If the exact answer is 2, then the numerical approximation is 2.0000000000. But let me check with a simple case. Suppose x=0 to 4, integrand x^{-1/2}(4 -x)^{-1/2} [1 -0.25x(4 -x)]^{1/2} dx. Let me plug in x=2. Then, the integrand is (2)^{-1/2}(2)^{-1/2} [1 -0.25*2)*(2)]^{1/2} = (1/√2)(1/√2) [1 -0.25*4]^{1/2} = (1/2) [1 -1]^{1/2} = 0. So at x=2, the integrand is 0. The function is symmetric around x=2. But integrating from 0 to4, the result is 2. Hmm, but let's check with another approach.

Alternatively, perhaps there's a substitution using trigonometric functions. Let me try x = 4 sin²θ. Wait, but x ranges from 0 to4, so maybe set x =4 sin²θ. Let’s try that. Let x =4 sin²θ, so dx =8 sinθ cosθ dθ. Then, when x=0, θ=0; x=4, θ=π/2. Then, the integrand becomes:

x^{-1/2} = (4 sin²θ)^{-1/2} = (1/(2 sinθ))

(4 -x)^{-1/2} = (4 -4 sin²θ)^{-1/2} = (4 cos²θ)^{-1/2} = 1/(2 cosθ)

The term inside the square root: 1 -0.25x(4 -x) =1 -0.25*4 sin²θ*4 cos²θ =1 -4 sin²θ cos²θ. Let's compute that:

4 sin²θ cos²θ = sin²(2θ). So, 1 - sin²(2θ) = cos²(2θ). Therefore, the square root is |cos(2θ)|. Since θ ranges from 0 to π/2, 2θ ranges from 0 to π. So, cos(2θ) is positive when θ in [0, π/4) and negative when θ in (π/4, π/2]. Therefore, |cos(2θ)| = cos(2θ) for θ in [0, π/4], and -cos(2θ) for θ in [π/4, π/2].

Putting it all together, the integrand becomes:

(1/(2 sinθ)) * (1/(2 cosθ)) * |cos(2θ)| *8 sinθ cosθ dθ

Simplify the terms:

(1/(4 sinθ cosθ)) * |cos(2θ)| *8 sinθ cosθ dθ = (8/4) |cos(2θ)| dθ = 2 |cos(2θ)| dθ.

Therefore, the integral becomes:

2 ∫₀^{π/2} |cos(2θ)| dθ.

Again, split the integral at θ=π/4 where cos(2θ) changes sign.

So, 2 [ ∫₀^{π/4} cos(2θ) dθ + ∫_{π/4}^{π/2} -cos(2θ) dθ ]

Compute each integral:

First integral: ∫ cos(2θ) dθ from 0 to π/4: (1/2) sin(2θ) from 0 to π/4 = (1/2)(sin(π/2) - sin(0)) = (1/2)(1 -0) = 1/2.

Second integral: ∫ -cos(2θ) dθ from π/4 to π/2: - (1/2) sin(2θ) ) from π/4 to π/2 = - (1/2)(sin(π) - sin(π/2)) = - (1/2)(0 -1) = 1/2.

So, total integral is 2*(1/2 +1/2) = 2*(1) =2. So, the integral is indeed 2. Therefore, the exact answer is 2. The numerical approximation is 2.0000000000.

But wait, let me confirm once more. The integral after substitution became 2 ∫₀^{π/2} |cos(2θ)| dθ = 2*(1/2 +1/2) =2*1=2. Yes. So, the exact value is 2. Therefore, the answer is 2, and numerically it's 2.0000000000.
</think>

{"answer": "2", "numerical_answer": "2.0000000000"}