We wish to evaluate

  I = ∫₀² x·arctan(√(x(2−x))) dx.

Step 1. Make a Trigonometric Substitution

Notice that
  x(2−x) = 2x − x².
A very useful substitution is
  x = 1 + cosθ.
Then
  2 − x = 2 − (1 + cosθ) = 1 − cosθ,
and hence
  x(2−x) = (1+cosθ)(1−cosθ) = 1 − cos²θ = sin²θ.
Thus,
  √(x(2−x)) = sinθ    (for 0 ≤ θ ≤ π, sinθ ≥ 0).
Also, differentiate: dx/dθ = − sinθ so that dx = − sinθ dθ.

Determine the limits:
  When x = 0:  0 = 1 + cosθ ⟹ cosθ = −1 ⟹ θ = π.
  When x = 2:  2 = 1 + cosθ ⟹ cosθ = 1 ⟹ θ = 0.

Substitute into the integral:
  I = ∫ₓ₌₀² x·arctan(√(x(2−x))) dx
    = ∫θ=π⁰ (1 + cosθ)·arctan(sinθ)(− sinθ dθ)
    = ∫₀π (1 + cosθ) sinθ · arctan(sinθ) dθ.

Step 2. Simplify the Integral

Write
  I = ∫₀π [1 + cosθ] sinθ · arctan(sinθ) dθ.
Split the integral as:
  I = ∫₀π sinθ·arctan(sinθ)dθ + ∫₀π cosθ·sinθ·arctan(sinθ)dθ.
Notice the second integrand. Make the substitution u = sinθ so that du = cosθ dθ. Then
  ∫₀π cosθ·sinθ·arctan(sinθ)dθ = ∫ u·arctan(u) du
evaluated from u = sin0 = 0 to u = sinπ = 0, so this integral is zero.

Thus, we are left with:
  I = ∫₀π sinθ·arctan(sinθ)dθ.

Step 3. Use Integration by Parts

Let
  u = arctan(sinθ)  ⟹ du = (cosθ/(1+sin²θ)) dθ,
  dv = sinθ dθ    ⟹ v = −cosθ.
Then, by integration by parts:
  I = [u v]₀π − ∫₀π v du
    = [ −cosθ·arctan(sinθ) ]₀π + ∫₀π cosθ·(cosθ/(1+sin²θ)) dθ.
Evaluate the boundary term:
  At θ = π: cosπ = −1, sinπ = 0, so −(−1)·arctan(0) = 0.
  At θ = 0: cos0 = 1, sin0 = 0, so −(1)·arctan(0) = 0.
Thus, the boundary term is 0 and we have:
  I = ∫₀π cos²θ/(1+ sin²θ) dθ.

Step 4. Simplify Further

Write cos²θ as 1 − sin²θ:
  I = ∫₀π [1 − sin²θ]/(1+ sin²θ) dθ.
Split this into two integrals:
  I = ∫₀π 1/(1+ sin²θ)dθ − ∫₀π sin²θ/(1+ sin²θ)dθ.
Notice that
  sin²θ/(1+ sin²θ) = 1 − 1/(1+ sin²θ).
Thus,
  ∫₀π sin²θ/(1+ sin²θ)dθ = ∫₀π 1 dθ − ∫₀π 1/(1+ sin²θ)dθ = π − ∫₀π 1/(1+ sin²θ)dθ.
So we obtain:
  I = ∫₀π 1/(1+ sin²θ)dθ − [π − ∫₀π 1/(1+ sin²θ)dθ]
    = 2∫₀π 1/(1+ sin²θ)dθ − π.

Step 5. Evaluate the Standard Integral

A standard result (which can be derived using the substitution u = cosθ) gives:
  ∫₀π dθ/(1+ sin²θ) = π/√2.
Therefore, we have:
  I = 2(π/√2) − π = (2π/√2) − π = π√2 − π = π(√2 − 1).

Step 6. Numerical Approximation

Since √2 ≈ 1.4142135623730950, then
  √2 − 1 ≈ 0.4142135623730950.
Multiplying by π (≈ 3.1415926535897930) we get:
  I ≈ 3.1415926535897930 × 0.4142135623730950 ≈ 1.3012902845685730.
Rounded to 10 decimal places, the numerical value is 1.3012902846.

Final Answer in JSON:
{"answer": "$\\pi(\\sqrt{2}-1)$", "numerical_answer": "1.3012902846"}