
To solve the definite integral \(\int\limits_0^1 \mathbf{L}_0(2\sqrt{x}) \mathbf{E}\left(\sqrt{1-x}\right) dx\), we proceed as follows:

### Step 1: Simplify the Integrand
The 0th Laguerre polynomial \(\mathbf{L}_0(x)\) is identically 1 for all \(x\). Thus, the integrand simplifies to \(\mathbf{E}\left(\sqrt{1-x}\right)\). The integral becomes:
\[
\int_0^1 \mathbf{E}\left(\sqrt{1-x}\right) dx
\]

### Step 2: Substitution
Let \(t = \sqrt{1-x}\), so \(x = 1 - t^2\) and \(dx = -2t \, dt\). When \(x = 0\), \(t = 1\); when \(x = 1\), \(t = 0\). Changing variables, the integral transforms to:
\[
\int_1^0 \mathbf{E}(t) \cdot (-2t) \, dt = \int_0^1 2t \, \mathbf{E}(t) \, dt
\]

### Step 3: Evaluate \(\int_0^1 2t \, \mathbf{E}(t) \, dt\)
We interchange the order of integration (justified by Fubiniâ€™s theorem) and use the definition of the complete elliptic integral of the second kind \(\mathbf{E}(t) = \int_0^{\pi/2} \sqrt{1 - t^2 \sin^2\theta} \, d\theta\). The integral becomes:
\[
\int_0^1 2t \left( \int_0^{\pi/2} \sqrt{1 - t^2 \sin^2\theta} \, d\theta \right) dt = \int_0^{\pi/2} \left( \int_0^1 2t \sqrt{1 - t^2 \sin^2\theta} \, dt \right) d\theta
\]

### Step 4: Inner Integral Over \(t\)
Let \(u = 1 - t^2 \sin^2\theta\), so \(du = -2t \sin^2\theta \, dt\). The inner integral transforms to:
\[
\int_{u=1}^{u=\cos^2\theta} \sqrt{u} \cdot \frac{-du}{\sin^2\theta} = \frac{1}{\sin^2\theta} \int_{\cos^2\theta}^1 \sqrt{u} \, du = \frac{2}{3 \sin^2\theta} \left(1 - \cos^3\theta\right)
\]

### Step 5: Integral Over \(\theta\)
The integral reduces to:
\[
\int_0^{\pi/2} \frac{2}{3 \sin^2\theta} \left(1 - \cos^3\theta\right) d\theta
\]
Simplifying \(\frac{1 - \cos^3\theta}{\sin^2\theta} = \cos\theta + \frac{1}{1 + \cos\theta}\) (using trigonometric identities), we split the integral:
\[
\frac{2}{3} \left( \int_0^{\pi/2} \cos\theta \, d\theta + \int_0^{\pi/2} \frac{1}{1 + \cos\theta} \, d\theta \right)
\]

### Step 6: Evaluate the Integrals
- \(\int_0^{\pi/2} \cos\theta \, d\theta = 1\)
- \(\int_0^{\pi/2} \frac{1}{1 + \cos\theta} \, d\theta = 1\) (using \(\frac{1}{1 + \cos\theta} = \frac{1}{2} \sec^2(\theta/2)\))

Thus, the integral becomes:
\[
\frac{2}{3} (1 + 1) = \frac{4}{3}
\]

### Numerical Approximation
The exact value is \(\frac{4}{3}\), which approximates to \(1.3333333333\) when rounded to 10 decimal places.

{"answer": "\\frac{4}{3}", "numerical_answer": "1.3333333333"}