Let's compute the definite integral:
\[
I = \int_0^1 x\:\mathbf{K}\left(\sqrt{x}\right)\mathbf{K}\left(\sqrt{1-x}\right) dx
\]
where \(\mathbf{K}(k)\) is the complete elliptic integral of the first kind.

---

### Step 1: Symmetry and Known Results

Recall a known result for the product of elliptic integrals:
\[
J = \int_0^1 \mathbf{K}\left(\sqrt{x}\right)\mathbf{K}\left(\sqrt{1-x}\right) dx = \frac{\pi^3}{8}
\]
But our integral has an extra \(x\) in the integrand.

Consider the symmetry:
Let \(y = 1-x\), then \(x \mathbf{K}\left(\sqrt{x}\right)\mathbf{K}\left(\sqrt{1-x}\right)\) becomes \((1-y)\mathbf{K}\left(\sqrt{1-y}\right)\mathbf{K}\left(\sqrt{y}\right)\) after interchanging \(x \leftrightarrow 1-x\).

Add the original and the transformed integral:
\[
I + I = \int_0^1 x \mathbf{K}(\sqrt{x})\mathbf{K}(\sqrt{1-x}) dx + \int_0^1 (1-x)\mathbf{K}(\sqrt{1-x})\mathbf{K}(\sqrt{x}) dx
\]
\[
= \int_0^1 \left[ x + (1-x) \right]\mathbf{K}(\sqrt{x})\mathbf{K}(\sqrt{1-x}) dx
\]
\[
= \int_0^1 \mathbf{K}(\sqrt{x})\mathbf{K}(\sqrt{1-x}) dx = J = \frac{\pi^3}{8}
\]

Therefore,
\[
2I = \frac{\pi^3}{8} \implies I = \frac{\pi^3}{16}
\]

---

### Step 2: Numerical Approximation

Calculate the value of \(\frac{\pi^3}{16}\):

First, \(\pi \approx 3.14159265358979\).
\[
\pi^3 = (3.14159265358979)^3 \approx 31.0062766802998
\]
\[
\frac{\pi^3}{16} \approx \frac{31.0062766802998}{16} \approx 1.9381422925
\]

---

### Step 3: Final Answer

```json
{"answer": "\\frac{\\pi^3}{16}", "numerical_answer": "1.9381422925"}
```