To solve the definite integral \(\int\limits_{0}^{2} x^{-1/2}(2-x)^{-1/2} \cosh\left(1 \sqrt{x(2-x)}\right) dx\), we will follow the steps outlined.

### Step 1: Analytical Computation

First, let's rewrite the integral for clarity:
\[ I = \int_{0}^{2} x^{-1/2}(2-x)^{-1/2} \cosh\left(\sqrt{x(2-x)}\right) dx. \]

We recognize that the integrand involves a hyperbolic cosine function and a product of two square roots. This suggests a possible substitution to simplify the integral.

Let \( t = \sqrt{x(2-x)} \). Then, we need to express \( dx \) in terms of \( dt \).

First, solve for \( x \) in terms of \( t \):
\[ t^2 = x(2 - x) \]
\[ t^2 = 2x - x^2 \]
\[ x^2 - 2x + t^2 = 0 \]

This is a quadratic equation in \( x \):
\[ x = \frac{2 \pm \sqrt{4 - 4t^2}}{2} = 1 \pm \sqrt{1 - t^2}. \]

Since \( x \) ranges from 0 to 2, we choose the appropriate branch:
\[ x = 1 + \sqrt{1 - t^2} \quad \text{or} \quad x = 1 - \sqrt{1 - t^2}. \]

We need to determine the limits of integration for \( t \). When \( x = 0 \):
\[ t = \sqrt{0 \cdot 2} = 0. \]

When \( x = 2 \):
\[ t = \sqrt{2 \cdot 0} = 0. \]

However, the maximum value of \( t \) occurs when \( x = 1 \):
\[ t = \sqrt{1 \cdot 1} = 1. \]

Thus, \( t \) ranges from 0 to 1.

Now, compute \( dx \) in terms of \( dt \):
\[ x = 1 + \sqrt{1 - t^2} \]
\[ dx = \frac{d}{dt} \left(1 + \sqrt{1 - t^2}\right) dt = \frac{-t}{\sqrt{1 - t^2}} dt. \]

Substitute \( x \) and \( dx \) back into the integral:
\[ I = \int_{0}^{1} \left(1 + \sqrt{1 - t^2}\right)^{-1/2} \left(1 - \sqrt{1 - t^2}\right)^{-1/2} \cosh(t) \left(\frac{-t}{\sqrt{1 - t^2}}\right) dt. \]

Simplify the integrand:
\[ \left(1 + \sqrt{1 - t^2}\right)^{-1/2} \left(1 - \sqrt{1 - t^2}\right)^{-1/2} = \left(1 - (1 - t^2)\right)^{-1/2} = t^{-1}. \]

Thus, the integral becomes:
\[ I = \int_{0}^{1} t^{-1} \cosh(t) \left(\frac{-t}{\sqrt{1 - t^2}}\right) dt = -\int_{0}^{1} \frac{\cosh(t)}{\sqrt{1 - t^2}} dt. \]

This integral is a standard form and can be evaluated using known results:
\[ \int_{0}^{1} \frac{\cosh(t)}{\sqrt{1 - t^2}} dt = \frac{\pi}{2} \cosh(1). \]

Thus,
\[ I = -\frac{\pi}{2} \cosh(1). \]

### Step 2: Numerical Approximation

To find the numerical approximation of \(-\frac{\pi}{2} \cosh(1)\), we use the values:
\[ \pi \approx 3.141592653589793, \]
\[ \cosh(1) \approx 1.543080634815244. \]

Thus,
\[ -\frac{\pi}{2} \cosh(1) \approx -\frac{3.141592653589793}{2} \times 1.543080634815244 \approx -2.427473042499859. \]

### Step 3: Final Answer in JSON Format

The exact answer in LaTeX is:
\[ -\frac{\pi}{2} \cosh(1). \]

The numerical approximation rounded to 10 decimal places is:
\[ -2.4274730425. \]

Thus, the final answer in the required JSON format is:
```json
{"answer": "-\\frac{\\pi}{2} \\cosh(1)", "numerical_answer": "-2.4274730425"}
```