

To calculate the definite integral \(\int_0^\infty \frac{1}{e^x + 1} \, dx\), we proceed as follows:

### Step 1: Substitution
Let \( t = e^x \). Then \( dt = e^x \, dx \), so \( dx = \frac{dt}{t} \). When \( x = 0 \), \( t = 1 \), and as \( x \to \infty \), \( t \to \infty \). The integral transforms to:
\[
\int_1^\infty \frac{1}{t(t + 1)} \, dt
\]

### Step 2: Partial Fraction Decomposition
Decompose \(\frac{1}{t(t + 1)}\) into partial fractions:
\[
\frac{1}{t(t + 1)} = \frac{1}{t} - \frac{1}{t + 1}
\]

### Step 3: Integrate Term by Term
The integral becomes:
\[
\int_1^\infty \left( \frac{1}{t} - \frac{1}{t + 1} \right) dt
\]
Integrate each term separately:
\[
\int \frac{1}{t} \, dt = \ln|t| \quad \text{and} \quad \int \frac{1}{t + 1} \, dt = \ln|t + 1|
\]

### Step 4: Evaluate the Definite Integral
Evaluate the antiderivative from \( t = 1 \) to \( t \to \infty \):
\[
\left[ \ln(t) - \ln(t + 1) \right]_1^\infty = \lim_{t \to \infty} \left( \ln\left( \frac{t}{t + 1} \right) \right) - \left( \ln(1) - \ln(2) \right)
\]
As \( t \to \infty \), \( \frac{t}{t + 1} \to 1 \), so \( \ln\left( \frac{t}{t + 1} \right) \to \ln(1) = 0 \). At \( t = 1 \), \( \ln(1) - \ln(2) = -\ln(2) \). Thus:
\[
0 - (-\ln(2)) = \ln(2)
\]

### Numerical Approximation
The numerical value of \( \ln(2) \) is approximately \( 0.69314718056 \), rounded to 10 decimal places: \( 0.6931471806 \).

{"answer": "\(\ln 2\)", "numerical_answer": "0.6931471806"}