
To solve the definite integral \(\int\limits_0^{2} x^{1/2}(2 - x)^{-1/2}\cos\left(\sqrt{x(2 - x)}\right)dx\), we proceed as follows:

### Step 1: Substitution
Let \(x = 1 + \sin\theta\). Then:
- When \(x = 0\), \(\theta = -\pi/2\); when \(x = 2\), \(\theta = \pi/2\).
- \(dx = \cos\theta \, d\theta\).
- \(x(2 - x) = 1 - \sin^2\theta = \cos^2\theta\), so \(\sqrt{x(2 - x)} = \cos\theta\).
- \(\sqrt{x}/\sqrt{2 - x} = \sqrt{(1 + \sin\theta)/(1 - \sin\theta)} = (1 + \sin\theta)/\cos\theta\) (after rationalizing).

The integral transforms to:
\[
\int_{-\pi/2}^{\pi/2} \left(\frac{1 + \sin\theta}{\cos\theta}\right) \cos(\cos\theta) \cdot \cos\theta \, d\theta = \int_{-\pi/2}^{\pi/2} (1 + \sin\theta)\cos(\cos\theta) \, d\theta.
\]

### Step 2: Simplifying the Integral
The integrand splits into two terms:
\[
\int_{-\pi/2}^{\pi/2} \cos(\cos\theta) \, d\theta + \int_{-\pi/2}^{\pi/2} \sin\theta \cos(\cos\theta) \, d\theta.
\]
The second integral involves an odd function over a symmetric interval, so it vanishes. The first integral involves an even function, so:
\[
\int_{-\pi/2}^{\pi/2} \cos(\cos\theta) \, d\theta = 2\int_0^{\pi/2} \cos(\cos\theta) \, d\theta.
\]

### Step 3: Relating to Bessel Functions
Using the integral representation of the Bessel function \(J_0(z)\):
\[
J_0(z) = \frac{1}{\pi} \int_0^\pi \cos(z \cos\theta) \, d\theta.
\]
For \(z = 1\), this gives:
\[
\int_0^\pi \cos(\cos\theta) \, d\theta = \pi J_0(1).
\]
Since \(2\int_0^{\pi/2} \cos(\cos\theta) \, d\theta = \int_0^\pi \cos(\cos\theta) \, d\theta\), the original integral simplifies to \(\pi J_0(1)\).

### Step 4: Numerical Approximation
The Bessel function \(J_0(1) \approx 0.7651976865579666\). Thus:
\[
\pi J_0(1) \approx 3.141592653589793 \times 0.7651976865579666 \approx 2.4039394433.
\]

### Final Answer
{"answer": "\(\pi J_0(1)\)", "numerical_answer": "2.4039394433"}