
To solve the definite integral \(\int\limits_0^1 x^{-1} \ln x \ln\frac{2+x}{2-x}\,dx\), we proceed as follows:


### Step 1: Simplify the Integrand
First, expand the logarithm of the quotient:
\[
\ln\frac{2+x}{2-x} = \ln(2+x) - \ln(2-x)
\]
Thus, the integral becomes:
\[
\int_0^1 \frac{\ln x}{x} \left[ \ln(2+x) - \ln(2-x) \right] dx
\]


### Step 2: Series Expansion of Logarithms
For \(|x| < 2\), we use the Taylor series expansion of \(\ln(2+x) - \ln(2-x)\). Rewrite the logarithms as:
\[
\ln(2+x) = \ln\left(2\left(1+\frac{x}{2}\right)\right) = \ln 2 + \ln\left(1+\frac{x}{2}\right)
\]
\[
\ln(2-x) = \ln\left(2\left(1-\frac{x}{2}\right)\right) = \ln 2 + \ln\left(1-\frac{x}{2}\right)
\]
Subtracting these, the \(\ln 2\) terms cancel, leaving:
\[
\ln(2+x) - \ln(2-x) = \ln\left(1+\frac{x}{2}\right) - \ln\left(1-\frac{x}{2}\right)
\]
Using the series for \(\ln(1+y) - \ln(1-y)\) (valid for \(|y| < 1\)):
\[
\ln\left(1+\frac{x}{2}\right) - \ln\left(1-\frac{x}{2}\right) = 2 \sum_{k=0}^\infty \frac{(x/2)^{2k+1}}{2k+1}
\]


### Step 3: Substitute the Series into the Integral
Substituting this series into the integral:
\[
\int_0^1 \frac{\ln x}{x} \cdot 2 \sum_{k=0}^\infty \frac{x^{2k+1}}{(2k+1)2^{2k+1}} dx = \sum_{k=0}^\infty \frac{1}{(2k+1)2^{2k}} \int_0^1 x^{2k} \ln x \, dx
\]


### Step 4: Evaluate the Inner Integral
The inner integral \(\int_0^1 x^{2k} \ln x \, dx\) is computed using integration by parts. Let \(u = \ln x\) and \(dv = x^{2k} dx\). Then \(du = \frac{1}{x} dx\) and \(v = \frac{x^{2k+1}}{2k+1}\). This gives:
\[
\int_0^1 x^{2k} \ln x \, dx = \left. \frac{x^{2k+1} \ln x}{2k+1} \right|_0^1 - \int_0^1 \frac{x^{2k}}{2k+1} dx = -\frac{1}{(2k+1)^2}
\]


### Step 5: Sum the Series
Substituting this result back, the integral becomes:
\[
\sum_{k=0}^\infty \frac{1}{(2k+1)2^{2k}} \left( -\frac{1}{(2k+1)^2} \right) = -\sum_{k=0}^\infty \frac{1}{(2k+1)^3 4^k}
\]


### Step 6: Numerical Approximation
The series \(\sum_{k=0}^\infty \frac{1}{(2k+1)^3 4^k}\) converges rapidly. Summing the first few terms (up to \(k=8\)) gives a numerical approximation of the series as \(1.009811047\). Thus, the integral is:
\[
-\sum_{k=0}^\infty \frac{1}{(2k+1)^3 4^k} \approx -1.009811047
\]


### Final Answer
The exact answer is expressed as a series involving polylogarithms, and the numerical approximation is approximately \(-1.009811047\).

```json
{"answer": "$-\\sum_{k=0}^{\\infty} \\frac{1}{(2k+1)^3 4^k}$", "numerical_answer": "-1.0098110470"}
```