We wish to evaluate
  I = ∫₀¹ (x²/(2 - x²) + √(2x/(x + 1))) dx.
We can split the integral as
  I = I₁ + I₂,
where

  I₁ = ∫₀¹ (x²/(2 - x²)) dx  and  I₂ = ∫₀¹ √(2x/(x + 1)) dx.

Step 1. Evaluation of I₁

Notice that
  x²/(2 - x²) = 2/(2 - x²) – 1,
since
  2/(2 - x²) – 1 = (2 – (2 – x²))/(2 - x²) = x²/(2 - x²).

Thus,
  I₁ = ∫₀¹ [2/(2 - x²) – 1] dx = 2∫₀¹ 1/(2 - x²) dx – ∫₀¹ dx.

The second integral is trivial: ∫₀¹ dx = 1.

To evaluate J = ∫₀¹ 1/(2 - x²) dx, use the substitution
  x = √2 sin θ  → dx = √2 cos θ dθ.
When x = 0, θ = 0; when x = 1, θ = arcsin(1/√2) = π/4.
The denominator transforms as:
  2 - x² = 2 - 2 sin²θ = 2 cos²θ.
Thus,
  J = ∫₀^(π/4) (√2 cos θ dθ)/(2 cos²θ) = (√2/2) ∫₀^(π/4) (1/cos θ)dθ = (1/√2) ∫₀^(π/4) sec θ dθ.
Recall that
  ∫ sec θ dθ = ln |sec θ + tan θ| + C.
Thus,
  J = (1/√2)[ln|sec θ + tan θ|]₀^(π/4)
At θ = π/4: sec(π/4) = √2 and tan(π/4) = 1, so ln(√2 + 1);
at θ = 0: sec 0 = 1 and tan 0 = 0, so ln 1 = 0.
Thus,
  J = (1/√2) ln(√2 + 1).
Returning to I₁:
  I₁ = 2J – 1 = 2(1/√2 ln(√2 + 1)) – 1 = √2 ln(√2 + 1) – 1.

Step 2. Evaluation of I₂

We now consider
  I₂ = ∫₀¹ √(2x/(x + 1)) dx.
Extract the constant under the square root:
  √(2x/(x+1)) = √2 · √(x/(x+1)).
Thus,
  I₂ = √2 · J₁, where J₁ = ∫₀¹ √(x/(x+1)) dx.

Now set t = √x so that x = t² and dx = 2t dt. Then,
  √(x/(x+1)) = t/√(t²+1).
Thus,
  J₁ = ∫₀¹ (t/√(t²+1)) · 2t dt = 2∫₀¹ (t²/√(t²+1)) dt.
Notice that t² = (t² + 1) – 1 so that
  t²/√(t²+1) = √(t²+1) – 1/√(t²+1).
Thus,
  J₁ = 2 [ ∫₀¹ √(t²+1) dt – ∫₀¹ 1/√(t²+1) dt ].

We use standard integrals:
  ∫ √(t²+1) dt = (t/2)√(t²+1) + (1/2) ln |t + √(t²+1)| + C,
  ∫ 1/√(t²+1) dt = asinh(t) = ln |t + √(t²+1)| + C.
Thus,
  ∫ √(t²+1) dt – ∫ 1/√(t²+1) dt = (t/2)√(t²+1) – (1/2) ln |t + √(t²+1)| + C.
Evaluate between 0 and 1:
At t = 1:
  (1/2)√2 – (1/2) ln(1+√2).
At t = 0:
  0 – (1/2) ln 1 = 0.
Thus, the difference equals:
  (√2)/2 – (1/2) ln(1+√2).
Multiplying by 2 gives:
  J₁ = 2[(√2)/2 – (1/2) ln(1+√2)] = √2 – ln(1+√2).

Returning to I₂:
  I₂ = √2 · (√2 – ln(1+√2)) = 2 – √2 ln(1+√2).

Step 3. Combine I₁ and I₂

Now, summing the two parts:
  I = I₁ + I₂ = [√2 ln(√2+1) – 1] + [2 – √2 ln(√2+1)] = 1.
Thus, the exact answer is 1.

Step 4. Numerical approximation

Numerically, 1 is exactly 1.0000000000 (to 10 decimal places).

The final answer in JSON format is:
{"answer": "1", "numerical_answer": "1.0000000000"}