To solve the definite integral \(\int_0^1 \frac{\ln(1 + x + x^2)}{x} \, dx\), we will follow the steps outlined.

### Step 1: Analytical Computation

First, we recognize that the integrand \(\frac{\ln(1 + x + x^2)}{x}\) can be simplified using a series expansion. We start by expanding \(\ln(1 + x + x^2)\) around \(x = 0\).

The function \(1 + x + x^2\) can be rewritten as:
\[ 1 + x + x^2 = \frac{1 - x^3}{1 - x} \]

Taking the natural logarithm of both sides, we get:
\[ \ln(1 + x + x^2) = \ln\left(\frac{1 - x^3}{1 - x}\right) = \ln(1 - x^3) - \ln(1 - x) \]

Using the series expansion for \(\ln(1 - u)\):
\[ \ln(1 - u) = -\sum_{n=1}^{\infty} \frac{u^n}{n} \]

We apply this to both \(\ln(1 - x^3)\) and \(\ln(1 - x)\):
\[ \ln(1 - x^3) = -\sum_{n=1}^{\infty} \frac{x^{3n}}{n} \]
\[ \ln(1 - x) = -\sum_{n=1}^{\infty} \frac{x^n}{n} \]

Thus,
\[ \ln(1 + x + x^2) = -\sum_{n=1}^{\infty} \frac{x^{3n}}{n} + \sum_{n=1}^{\infty} \frac{x^n}{n} \]

Now, we substitute this back into the integral:
\[ \int_0^1 \frac{\ln(1 + x + x^2)}{x} \, dx = \int_0^1 \frac{1}{x} \left( -\sum_{n=1}^{\infty} \frac{x^{3n}}{n} + \sum_{n=1}^{\infty} \frac{x^n}{n} \right) dx \]

We can interchange the summation and integration:
\[ \int_0^1 \frac{\ln(1 + x + x^2)}{x} \, dx = -\sum_{n=1}^{\infty} \frac{1}{n} \int_0^1 x^{3n-1} \, dx + \sum_{n=1}^{\infty} \frac{1}{n} \int_0^1 x^{n-1} \, dx \]

Evaluating the integrals:
\[ \int_0^1 x^{3n-1} \, dx = \frac{1}{3n} \]
\[ \int_0^1 x^{n-1} \, dx = \frac{1}{n} \]

Thus,
\[ \int_0^1 \frac{\ln(1 + x + x^2)}{x} \, dx = -\sum_{n=1}^{\infty} \frac{1}{n} \cdot \frac{1}{3n} + \sum_{n=1}^{\infty} \frac{1}{n} \cdot \frac{1}{n} \]
\[ = -\sum_{n=1}^{\infty} \frac{1}{3n^2} + \sum_{n=1}^{\infty} \frac{1}{n^2} \]
\[ = \sum_{n=1}^{\infty} \frac{1}{n^2} - \frac{1}{3} \sum_{n=1}^{\infty} \frac{1}{n^2} \]
\[ = \left(1 - \frac{1}{3}\right) \sum_{n=1}^{\infty} \frac{1}{n^2} \]
\[ = \frac{2}{3} \sum_{n=1}^{\infty} \frac{1}{n^2} \]

We know that \(\sum_{n=1}^{\infty} \frac{1}{n^2} = \frac{\pi^2}{6}\), so:
\[ \int_0^1 \frac{\ln(1 + x + x^2)}{x} \, dx = \frac{2}{3} \cdot \frac{\pi^2}{6} = \frac{\pi^2}{9} \]

### Step 2: Numerical Approximation

To find the numerical approximation of \(\frac{\pi^2}{9}\), we use the value of \(\pi \approx 3.141592653589793\):
\[ \frac{\pi^2}{9} \approx \frac{(3.141592653589793)^2}{9} \approx \frac{9.869604401089358}{9} \approx 1.0962893778988176 \]

Rounded to 10 decimal places, this is:
\[ 1.0962893779 \]

### Step 3: Final Answer in JSON Format

```json
{"answer": "\\frac{\\pi^2}{9}", "numerical_answer": "1.0962893779"}
```