Let's denote the integral as:
\[
I = \int_0^6 x + (x-3)^7 + \sin(x-3) \, dx
\]

Let's break it into three parts:
\[
I = \int_0^6 x \, dx + \int_0^6 (x-3)^7 \, dx + \int_0^6 \sin(x-3) \, dx
\]

---

### 1. Compute each part analytically

#### a) \(\int_0^6 x \, dx\):

\[
\int x \, dx = \frac{1}{2}x^2
\]
Evaluate from 0 to 6:
\[
\left. \frac{1}{2}x^2 \right|_0^6 = \frac{1}{2}(6^2) - \frac{1}{2}(0^2) = \frac{1}{2}(36) = 18
\]

---

#### b) \(\int_0^6 (x-3)^7 dx\)

Let \(u = x-3 \implies dx = du\).
When \(x = 0\), \(u = -3\). When \(x = 6\), \(u = 3\).
So,
\[
\int_0^6 (x-3)^7 dx = \int_{-3}^{3} u^7 du
\]
\[
\int u^7 du = \frac{1}{8}u^8
\]
\[
\left. \frac{1}{8}u^8 \right|_{-3}^{3} = \frac{1}{8}(3^8 - (-3)^8)
\]
\[
(-3)^8 = 3^8 \Rightarrow 3^8 - 3^8 = 0
\]
So this term is \(0\).

---

#### c) \(\int_0^6 \sin(x-3) dx\)

Let \(u = x-3 \implies dx = du\), as above.
When \(x = 0\), \(u = -3\). When \(x = 6\), \(u = 3\).
So,
\[
\int_0^6 \sin(x-3) dx = \int_{-3}^3 \sin(u) du
\]
\[
\int \sin u \, du = -\cos u
\]
So,
\[
\left. -\cos u \right|_{-3}^3 = -\cos(3) + \cos(-3)
\]
But \(\cos(-3) = \cos(3)\), since cosine is an even function.

Thus,
\[
-\cos(3) + \cos(3) = 0
\]

---

So, only the first term remains.

## 2. Exact Answer

\[
I = 18
\]

---

## 3. Numerical Approximation (rounded to 10 decimal places)

\[
I \approx 18.0000000000
\]

---

## 4. Final Answer (JSON)

```json
{"answer": "18", "numerical_answer": "18.0000000000"}
```