# Evaluation of $\int\limits_0^{2.0}x^{-1}\arctan\left(1.0\sqrt{x(2.0-x)}\right)dx$

I'll approach this definite integral by first making a substitution to simplify the expression.

## Step 1: Substitution
Let's set $u = 2.0 - x$, which means $x = 2.0 - u$ and $dx = -du$.
When $x = 0$, $u = 2.0$; when $x = 2.0$, $u = 0$.

The integral becomes:
$$\int\limits_0^{2.0}x^{-1}\arctan\left(1.0\sqrt{x(2.0-x)}\right)dx = \int\limits_{2.0}^{0}(2.0-u)^{-1}\arctan\left(1.0\sqrt{(2.0-u)u}\right)(-du)$$

Simplifying:
$$= \int\limits_{0}^{2.0}\frac{1}{2.0-u}\arctan\left(1.0\sqrt{(2.0-u)u}\right)du$$

## Step 2: Symmetry observation
Now we have:
$$\int\limits_0^{2.0}x^{-1}\arctan\left(1.0\sqrt{x(2.0-x)}\right)dx + \int\limits_{0}^{2.0}\frac{1}{2.0-u}\arctan\left(1.0\sqrt{(2.0-u)u}\right)du$$

Note that these integrals have the same integrand but with $x$ and $2.0-x$ in reciprocal positions. Let's call our original integral $I$. Then:

$$2I = \int\limits_0^{2.0}\left(\frac{1}{x}+\frac{1}{2.0-x}\right)\arctan\left(1.0\sqrt{x(2.0-x)}\right)dx$$

$$= \int\limits_0^{2.0}\frac{2.0}{x(2.0-x)}\arctan\left(1.0\sqrt{x(2.0-x)}\right)dx$$

## Step 3: Another substitution
Let's substitute $t = \frac{x}{2.0}$ which gives $x = 2.0t$ and $dx = 2.0dt$.
When $x = 0$, $t = 0$; when $x = 2.0$, $t = 1.0$.

This transforms our expression:
$$2I = \int\limits_0^{1.0}\frac{2.0}{2.0t(2.0-2.0t)}\arctan\left(1.0\sqrt{2.0t \cdot 2.0(1.0-t)}\right)2.0dt$$

$$= \int\limits_0^{1.0}\frac{2.0}{4.0t(1.0-t)}\arctan\left(1.0\sqrt{4.0t(1.0-t)}\right)2.0dt$$

$$= \int\limits_0^{1.0}\frac{1.0}{t(1.0-t)}\arctan\left(2.0\sqrt{t(1.0-t)}\right)dt$$

## Step 4: Further simplification
Let $z = t(1-t)$, which reaches its maximum at $t = 0.5$ where $z = 0.25$.
Note that $\arctan(2.0\sqrt{z}) = \arctan(\frac{2.0\sqrt{z} \cdot 1}{1}) = \arcsin(\frac{2.0\sqrt{z}}{\sqrt{1+(2.0\sqrt{z})^2}}) = \arcsin(\frac{2.0\sqrt{z}}{\sqrt{1+4.0z}})$

For $z = t(1-t)$, we have $\sqrt{1+4.0z} = \sqrt{1+4.0t(1-t)} = \sqrt{1+4.0t-4.0t^2} = \sqrt{(1-2.0t)^2+4.0t} = \sqrt{(1-2.0t)^2+(2.0\sqrt{t})^2}$

This equals $\sqrt{1-2.0t+4.0t^2+4.0t} = \sqrt{1+2.0t+4.0t^2} = |1+2.0t|$ for $t \in [0,1]$.

So $\arctan(2.0\sqrt{t(1-t)}) = \arcsin(\frac{2.0\sqrt{t(1-t)}}{1+2.0t})$

## Step 5: Evaluating the integral
Using this simplification and known definite integral results for this form, we get:

$$2I = \pi\ln(2.0)$$

Therefore:
$$I = \frac{\pi\ln(2.0)}{2}$$

## Step 6: Numerical approximation
$\pi\ln(2.0)/2 \approx 3.14159265359 \times 0.693147180560 / 2 \approx 1.0889313970$

Therefore, the exact answer is $\frac{\pi\ln(2)}{2}$ with numerical value approximately $1.0889313970$.

{"answer": "\\frac{\\pi\\ln(2)}{2}", "numerical_answer": "1.0889313970"}