

To solve the definite integral \(\int_1^2 \frac{9x + 4}{x^5 + 3x^2 + x} \, dx\), we follow these steps:

### Step 1: Factor the Denominator
The denominator \(x^5 + 3x^2 + x\) can be factored as \(x(x^4 + 3x + 1)\).

### Step 2: Partial Fraction Decomposition
We decompose the integrand into partial fractions. Let:
\[
\frac{9x + 4}{x(x^4 + 3x + 1)} = \frac{A}{x} + \frac{Bx^3 + Cx^2 + Dx + E}{x^4 + 3x + 1}
\]
Multiplying both sides by \(x(x^4 + 3x + 1)\) and equating coefficients, we find \(A = 4\), \(B = -4\), \(C = 0\), \(D = 0\), and \(E = -3\). Thus:
\[
\frac{9x + 4}{x(x^4 + 3x + 1)} = \frac{4}{x} - \frac{4x^3 + 3}{x^4 + 3x + 1}
\]

### Step 3: Integrate Term by Term
The integral splits into two parts:
\[
\int \left( \frac{4}{x} - \frac{4x^3 + 3}{x^4 + 3x + 1} \right) dx
\]
- The first term integrates to \(4 \ln|x|\).
- The second term has a numerator that is the derivative of the denominator (\(d/dx(x^4 + 3x + 1) = 4x^3 + 3\)), so it integrates to \(-\ln|x^4 + 3x + 1|\).

### Step 4: Evaluate the Definite Integral
Combining these results, the antiderivative is:
\[
F(x) = 4 \ln x - \ln(x^4 + 3x + 1)
\]
Evaluating from \(1\) to \(2\):
\[
F(2) - F(1) = \left[4 \ln 2 - \ln(2^4 + 3 \cdot 2 + 1)\right] - \left[4 \ln 1 - \ln(1^4 + 3 \cdot 1 + 1)\right]
\]
Simplifying:
\[
= 4 \ln 2 - \ln 23 - (0 - \ln 5) = 4 \ln 2 + \ln 5 - \ln 23 = \ln\left(\frac{80}{23}\right)
\]

### Step 5: Numerical Approximation
The exact value is \(\ln\left(\frac{80}{23}\right)\). Numerically, \(\frac{80}{23} \approx 3.47826087\), and \(\ln(3.47826087) \approx 1.2469262359\).

{"answer": "\(\ln\left(\frac{80}{23}\right)\)", "numerical_answer": "1.2469262359"}