


To solve the definite integral \(\int\limits_0^1 x\arccos x\, I_0(2x)\,dx\), we proceed as follows:

### Step 1: Series Expansion of \(I_0(2x)\)
The modified Bessel function of the first kind of order zero, \(I_0(z)\), has the series expansion:
\[
I_0(z) = \sum_{n=0}^\infty \frac{(z^2/4)^n}{(n!)^2}
\]
For \(z = 2x\), this becomes:
\[
I_0(2x) = \sum_{n=0}^\infty \frac{x^{2n}}{(n!)^2}
\]

### Step 2: Integral as a Series
Substituting the series into the integral, we get:
\[
\int_0^1 x\arccos x\, I_0(2x)\,dx = \sum_{n=0}^\infty \frac{1}{(n!)^2} \int_0^1 x^{2n+1} \arccos x\,dx
\]

### Step 3: Integrate \(x^{2n+1} \arccos x\)
We use integration by parts on \(\int x^{2n+1} \arccos x\,dx\). Let \(u = \arccos x\) and \(dv = x^{2n+1}dx\). Then \(du = -\frac{1}{\sqrt{1-x^2}}dx\) and \(v = \frac{x^{2n+2}}{2n+2}\). Applying integration by parts:
\[
\int x^{2n+1} \arccos x\,dx = \left. \frac{x^{2n+2}}{2n+2} \arccos x \right|_0^1 + \frac{1}{2n+2} \int_0^1 \frac{x^{2n+2}}{\sqrt{1-x^2}}dx
\]
The boundary term vanishes (since \(\arccos 1 = 0\) and \(x^{2n+2} = 0\) at \(x=0\)), leaving:
\[
\int_0^1 x^{2n+1} \arccos x\,dx = \frac{1}{2n+2} \int_0^1 \frac{x^{2n+2}}{\sqrt{1-x^2}}dx
\]

### Step 4: Evaluate \(\int_0^1 \frac{x^{2n+2}}{\sqrt{1-x^2}}dx\)
Using the substitution \(t = x^2\) (so \(x = \sqrt{t}\), \(dx = \frac{1}{2\sqrt{t}}dt\)), the integral becomes:
\[
\int_0^1 \frac{t^{n+1}}{\sqrt{1-t}} \cdot \frac{1}{2\sqrt{t}}dt = \frac{1}{2} \int_0^1 t^{n+\frac{1}{2}} (1-t)^{-\frac{1}{2}}dt
\]
This is a Beta function: \(\frac{1}{2} B\left(n+\frac{3}{2}, \frac{1}{2}\right)\). Using \(B(a,b) = \frac{\Gamma(a)\Gamma(b)}{\Gamma(a+b)}\) and \(\Gamma\left(\frac{1}{2}\right) = \sqrt{\pi}\), we get:
\[
\int_0^1 \frac{x^{2n+2}}{\sqrt{1-x^2}}dx = \frac{\sqrt{\pi}}{2} \cdot \frac{\Gamma\left(n+\frac{3}{2}\right)}{\Gamma(n+2)}
\]

### Step 5: Combine Results
Substituting back, the original integral becomes:
\[
\int_0^1 x\arccos x\, I_0(2x)\,dx = \sum_{n=0}^\infty \frac{\sqrt{\pi}}{2(2n+2)(n!)^2} \cdot \frac{\Gamma\left(n+\frac{3}{2}\right)}{\Gamma(n+2)}
\]
Simplifying \(\Gamma(n+2) = (n+1)!\) and \(\Gamma\left(n+\frac{3}{2}\right) = \frac{(2n+2)!\sqrt{\pi}}{4^{n+1}(n+1)!}}\), the series simplifies to a sum of terms involving \(\pi\) and factorials.

### Step 6: Numerical Approximation
The series converges rapidly. Summing the first few terms (up to \(n=4\)) gives a numerical approximation of approximately \(0.561972\).


### Final Answer
The exact answer is the series sum, and the numerical approximation is:

{"answer": "\\sum_{n=0}^{\\infty} \\frac{\\pi (2n + 2)!}{4^{n + 2} (n + 1)^2 (n!)^3 (n + 1)!}", "numerical_answer": "0.5619720000"}