<think>
Okay, let's tackle this integral step by step. The integral given is from 0 to 1 of (x²/(2 - x²) + sqrt(2x/(x + 1))) dx. Hmm, so it's the sum of two functions, so maybe I can split the integral into two separate parts. That should make things easier. Let me write that down:

∫₀¹ [x²/(2 - x²) + sqrt(2x/(x + 1))] dx = ∫₀¹ x²/(2 - x²) dx + ∫₀¹ sqrt(2x/(x + 1)) dx

Alright, let's handle each integral one by one.

Starting with the first integral: ∫ x²/(2 - x²) dx. Hmm, the denominator is 2 - x², and the numerator is x². Maybe I can help here. Let me try to manipulate the numerator to make it look like the denominator. If I rewrite the numerator as (2 - x²) - 2, that might work. Let's see:

x² = -(2 - x²) + 2. Wait, let's check:

If I take 2 - x² and subtract that from 2, I get 2 - (2 - x²) = x². Wait, no. Wait, maybe I should rearrange:

Let me think. Let's express x² as (2 - x²) - 2 ) multiplied by -1. Let's see:

x² = -( (2 - x²) - 2 ) = - (2 - x²) + 2. Yes, that's correct. So then:

x²/(2 - x²) = [ - (2 - x²) + 2 ] / (2 - x²) = -1 + 2/(2 - x²)

So the integral becomes ∫ (-1 + 2/(2 - x²)) dx. That's much simpler! So integrating term by term:

∫ -1 dx + ∫ 2/(2 - x²) dx

The first integral is straightforward: -x evaluated from 0 to 1. The second integral is 2/(2 - x²). The integral of 1/(a² - x²) dx is (1/(2a)) ln |(a + x)/(a - x)| + C. So here, a² = 2, so a = sqrt(2). Therefore:

∫ 2/(2 - x²) dx = 2 * [1/(2 sqrt(2)) ln |(sqrt(2) + x)/(sqrt(2) - x)| ] + C = (1/sqrt(2)) ln |(sqrt(2) + x)/(sqrt(2) - x)| + C

So putting it all together, the first integral from 0 to 1 is:

[ -x + (1/sqrt(2)) ln((sqrt(2) + x)/(sqrt(2) - x)) ] evaluated from 0 to 1.

Wait, no. Wait, the first term is ∫ -1 dx, which is -x. Then the second term is the logarithmic part. So the entire first integral is:

[-x + (1/sqrt(2)) ln((sqrt(2) + x)/(sqrt(2) - x))] from 0 to 1.

Let's compute that. At x = 1:

-1 + (1/sqrt(2)) ln( (sqrt(2) + 1)/(sqrt(2) - 1) )

At x = 0:

-0 + (1/sqrt(2)) ln( (sqrt(2) + 0)/(sqrt(2) - 0) ) = (1/sqrt(2)) ln(1) = 0

So the first integral evaluates to:

[ -1 + (1/sqrt(2)) ln( (sqrt(2) + 1)/(sqrt(2) - 1) ) ] - 0

Simplify the logarithmic term. Let's note that (sqrt(2) + 1)/(sqrt(2) - 1) can be rationalized. Multiply numerator and denominator by (sqrt(2) + 1):

[(sqrt(2) + 1)^2] / [ (sqrt(2))^2 - 1^2 ] = ( (2 + 2 sqrt(2) + 1 ) ) / (2 - 1) ) = (3 + 2 sqrt(2))/1 = 3 + 2 sqrt(2)

So ln( (sqrt(2) + 1)/(sqrt(2) - 1) ) = ln(3 + 2 sqrt(2))

But 3 + 2 sqrt(2) is actually (sqrt(2) + 1)^2. Let me check:

(sqrt(2) + 1)^2 = 2 + 2 sqrt(2) + 1 = 3 + 2 sqrt(2). Yes, correct. So ln( (sqrt(2) + 1)^2 ) = 2 ln(sqrt(2) + 1). Therefore, the expression becomes:

-1 + (1/sqrt(2)) * 2 ln(sqrt(2) + 1) = -1 + (2/sqrt(2)) ln(sqrt(2) + 1)

Simplify 2/sqrt(2) = sqrt(2). So:

-1 + sqrt(2) ln(sqrt(2) + 1)

So that's the result of the first integral. Alright, moving on to the second integral: ∫₀¹ sqrt(2x/(x + 1)) dx.

Let me make a substitution here. Let u = 2x/(x + 1). Wait, but that might complicate. Alternatively, maybe substitute t = sqrt(2x/(x + 1)). Let me see. Let me try to simplify the expression inside the square root first.

sqrt(2x/(x + 1)) can be written as sqrt(2) * (x/(x + 1))^(1/2). Hmm, perhaps substitution. Let me set t = x/(x + 1). Then, x = t/(1 - t). Wait, maybe that's not the best approach. Alternatively, let me set u = x + 1. Then du = dx, and x = u - 1. Let's try that.

But when x = 0, u = 1; when x = 1, u = 2. The integral becomes:

sqrt(2(u - 1)/u) * du from u=1 to u=2.

Simplify inside the square root: 2(u - 1)/u = 2(1 - 1/u). So sqrt(2(1 - 1/u)) = sqrt(2) * sqrt(1 - 1/u). Hmm, not sure if that helps. Maybe another substitution. Let me think.

Alternatively, let me set t = sqrt(2x/(x + 1)). Let's square both sides: t² = 2x/(x + 1). Then, multiply both sides by (x + 1):

t²(x + 1) = 2x => t² x + t² = 2x => t² = 2x - t² x => t² = x(2 - t²) => x = t²/(2 - t²)

Then, dx/dt = [2t(2 - t²) - t²(-2t)]/(2 - t²)^2 = [4t - 2t³ + 2t³]/(2 - t²)^2 = 4t/(2 - t²)^2

So dx = 4t/(2 - t²)^2 dt

Now, when x = 0, t = 0. When x = 1, t² = 2*1)/(1 + 1) = 2/2 = 1, so t = 1. So the limits are from t=0 to t=1.

So the integral becomes ∫₀¹ t * [4t/(2 - t²)^2] dt = 4 ∫₀¹ t²/(2 - t²)^2 dt

Hmm, that seems more complicated. Maybe there's a better substitution. Let me think again.

Alternatively, let's try to rationalize the integrand. Let me write sqrt(2x/(x + 1)) as sqrt(2x)/sqrt(x + 1). Let me set u = sqrt(x + 1). Then, u² = x + 1 => x = u² - 1, so dx = 2u du. Then, when x = 0, u = 1; x = 1, u = sqrt(2). The integral becomes:

sqrt(2(u² - 1))/u * 2u du = sqrt(2) * sqrt(u² - 1) * 2 du

Simplify: 2 sqrt(2) * sqrt(u² - 1) du, integrated from u=1 to u=sqrt(2).

Hmm, that's better. The integral of sqrt(u² - 1) du is known. The standard integral ∫ sqrt(u² - a²) du = (u/2) sqrt(u² - a²) - (a²/2) ln(u + sqrt(u² - a²)) ) + C. Here, a = 1. So:

∫ sqrt(u² - 1) du = (u/2) sqrt(u² - 1) - (1/2) ln(u + sqrt(u² - 1)) ) + C

Therefore, our integral becomes:

2 sqrt(2) [ (u/2) sqrt(u² - 1) - (1/2) ln(u + sqrt(u² - 1)) ) ] evaluated from 1 to sqrt(2)

Simplify the coefficients:

2 sqrt(2) * [ (u sqrt(u² - 1)/2 - (1/2) ln(u + sqrt(u² - 1)) ) ]

= sqrt(2) [ u sqrt(u² - 1) - ln(u + sqrt(u² - 1)) ] from 1 to sqrt(2)

Now evaluate at the limits:

First, at u = sqrt(2):

sqrt(2) [ sqrt(2) * sqrt( (sqrt(2))² - 1 ) - ln( sqrt(2) + sqrt( (sqrt(2))² - 1 ) ) ]

Compute sqrt(2)² - 2 = 2 - 1 = 1. So sqrt(1) = 1. Therefore:

sqrt(2) [ sqrt(2) * 1 - ln( sqrt(2) + 1 ) ] = sqrt(2) [ sqrt(2) - ln(sqrt(2) + 1) ] = 2 - sqrt(2) ln(sqrt(2) + 1)

At u = 1:

sqrt(2) [ 1 * sqrt(1 - 1) - ln(1 + sqrt(0)) ] = sqrt(2) [0 - ln(1 + 0) ] = sqrt(2) [0 - 0] = 0

So the entire second integral evaluates to:

[2 - sqrt(2) ln(sqrt(2) + 1)] - 0 = 2 - sqrt(2) ln(sqrt(2) + 1)

So combining both integrals:

First integral result: -1 + sqrt(2) ln(sqrt(2) + 1)

Second integral result: 2 - sqrt(2) ln(sqrt(2) + 1)

Adding them together:

(-1 + sqrt(2) ln(sqrt(2) + 1)) + (2 - sqrt(2) ln(sqrt(2) + 1)) = (-1 + 2) + (sqrt(2) ln(...) - sqrt(2) ln(...)) = 1 + 0 = 1

Wait, that's interesting! The terms with the logarithm cancel out, leaving just 1. So the total integral from 0 to 1 is 1?

Wait, that seems surprisingly simple. Let me check my steps again to make sure I didn't make a mistake.

First integral:

∫₀¹ x²/(2 - x²) dx = -1 + sqrt(2) ln(sqrt(2) + 1)

Second integral:

∫₀¹ sqrt(2x/(x + 1)) dx = 2 - sqrt(2) ln(sqrt(2) + 1)

Adding them: (-1 + sqrt(2) ln(...)) + (2 - sqrt(2) ln(...)) = (-1 + 2) + (sqrt(2) ln(...) - sqrt(2) ln(...)) = 1 + 0 = 1

So the exact value is 1? That's unexpected but seems correct. Let me verify with a numerical approximation.

Let's compute the numerical value. Let's first compute the first integral's contribution:

First integral: -1 + sqrt(2) * ln(sqrt(2) + 1)

sqrt(2) ≈ 1.41421356237

ln(sqrt(2) + 1) ≈ ln(1.41421356237 + 1) = ln(2.41421356237) ≈ 0.88137358702

So sqrt(2) * 0.88137358702 ≈ 1.41421356237 * 0.88137358702 ≈ 1.24645048

Then subtract 1: 1.24645048 - 1 = 0.24645048

Second integral: 2 - sqrt(2) * ln(sqrt(2) + 1) ≈ 2 - 1.24645048 ≈ 0.75354952

Adding them: 0.24645048 + 0.75354952 ≈ 1.0

So numerically, it's 1.0. So the exact answer is 1. That's a neat result. So the definite integral from 0 to 1 of that expression is exactly 1.

Therefore, the exact answer is 1, and the numerical approximation is 1.0000000000. But let me check with another method to be sure.

Alternatively, maybe there's a trick to see that the sum of the derivative of some function. But given that the analytical steps led to cancellation, and the numerical check gives 1, it's safe to conclude the exact answer is 1.

So the final answer is 1. The exact answer is 1, and the numerical approximation is 1.0000000000.
</think>

{"answer": "1", "numerical_answer": "1.0000000000"}