# Evaluating $\int_0^{\pi/4}\frac{\tan(x)+2\sec^2(x)+2\tan(x)\sec^2(x)}{\tan(x)+\sec^2(x)}\text{ dx}$

## Step 1: Simplify the integrand

Let's work on simplifying the expression in the integrand:

$$\frac{\tan(x)+2\sec^2(x)+2\tan(x)\sec^2(x)}{\tan(x)+\sec^2(x)}$$

I'll factor out common terms in the numerator:

$$\frac{\tan(x) + 2\sec^2(x) + 2\tan(x)\sec^2(x)}{\tan(x)+\sec^2(x)} = \frac{\tan(x)(1 + 2\sec^2(x)) + 2\sec^2(x)}{\tan(x)+\sec^2(x)}$$

Now, I'll try a different approach. Let's denote $u = \tan(x)$ and $v = \sec^2(x)$. Note that $v = 1 + u^2$ since $\sec^2(x) = 1 + \tan^2(x)$.

The integrand becomes:
$$\frac{u + 2v + 2uv}{u + v}$$

Let's expand this:
$$\frac{u + 2v + 2uv}{u + v} = \frac{u + 2v + 2u(1+u^2)}{u + v}$$

Actually, let's go back to the original approach and try to simplify directly:

$$\frac{\tan(x) + 2\sec^2(x) + 2\tan(x)\sec^2(x)}{\tan(x)+\sec^2(x)}$$

I'll perform a polynomial division:

$$\frac{\tan(x) + 2\sec^2(x) + 2\tan(x)\sec^2(x)}{\tan(x)+\sec^2(x)} = \frac{\tan(x) + 2\sec^2(x)(1 + \tan(x))}{\tan(x)+\sec^2(x)}$$

Let's continue with the division:
$$\begin{align*}
\frac{\tan(x) + 2\sec^2(x)(1 + \tan(x))}{\tan(x)+\sec^2(x)} &= \frac{\tan(x) + 2\sec^2(x) + 2\sec^2(x)\tan(x)}{\tan(x)+\sec^2(x)}\\
\end{align*}$$

Let me try another approach. Let's define $f(x) = \tan(x) + \sec^2(x)$. Then our integrand becomes:

$$\frac{\tan(x) + 2\sec^2(x) + 2\tan(x)\sec^2(x)}{f(x)}$$

Now, observe that:
$$\begin{align*}
\frac{d}{dx}[f(x)] &= \frac{d}{dx}[\tan(x) + \sec^2(x)]\\
&= \sec^2(x) + 2\sec(x)\tan(x)\frac{d}{dx}[\sec(x)]\\
&= \sec^2(x) + 2\sec(x)\tan(x) \cdot \sec(x)\tan(x)\\
&= \sec^2(x) + 2\sec^2(x)\tan^2(x)\\
&= \sec^2(x)(1 + 2\tan^2(x))
\end{align*}$$

This doesn't match our numerator perfectly, so let's try a different approach.

Let me try direct algebraic manipulation:

$$\begin{align*}
\frac{\tan(x) + 2\sec^2(x) + 2\tan(x)\sec^2(x)}{\tan(x)+\sec^2(x)} &= \frac{\tan(x) + 2\sec^2(x) + 2\tan(x)\sec^2(x)}{\tan(x)+\sec^2(x)}\\
\end{align*}$$

Let's try factoring:
$$\begin{align*}
\frac{\tan(x) + 2\sec^2(x) + 2\tan(x)\sec^2(x)}{\tan(x)+\sec^2(x)} &= \frac{\tan(x)(1 + 2\sec^2(x)) + 2\sec^2(x)}{\tan(x)+\sec^2(x)}\\
\end{align*}$$

I'll try yet another approach. Let's use the fact that $\sec^2(x) = 1 + \tan^2(x)$:

$$\begin{align*}
\frac{\tan(x) + 2\sec^2(x) + 2\tan(x)\sec^2(x)}{\tan(x)+\sec^2(x)} &= \frac{\tan(x) + 2(1 + \tan^2(x)) + 2\tan(x)(1 + \tan^2(x))}{\tan(x)+(1 + \tan^2(x))}\\
&= \frac{\tan(x) + 2 + 2\tan^2(x) + 2\tan(x) + 2\tan^3(x)}{1 + \tan(x) + \tan^2(x)}\\
&= \frac{3\tan(x) + 2 + 2\tan^2(x) + 2\tan^3(x)}{1 + \tan(x) + \tan^2(x)}\\
\end{align*}$$

Let's set $u = \tan(x)$ to simplify:

$$\begin{align*}
\frac{3u + 2 + 2u^2 + 2u^3}{1 + u + u^2}
\end{align*}$$

Now, let's perform polynomial long division:

$$(3u + 2 + 2u^2 + 2u^3) \div (1 + u + u^2)$$

We get:
$$2u + 1 + \frac{2}{1 + u + u^2}$$

So our integrand simplifies to:
$$\frac{\tan(x) + 2\sec^2(x) + 2\tan(x)\sec^2(x)}{\tan(x)+\sec^2(x)} = 2\tan(x) + 1 + \frac{2}{1 + \tan(x) + \tan^2(x)}$$

## Step 2: Integrate the simplified expression

$$\int_0^{\pi/4}\left(2\tan(x) + 1 + \frac{2}{1 + \tan(x) + \tan^2(x)}\right) dx$$

Let's integrate each term:

1. $\int 2\tan(x) dx = -2\ln|\cos(x)| + C$
2. $\int 1 dx = x + C$
3. For $\int \frac{2}{1 + \tan(x) + \tan^2(x)} dx$, we need to use substitution.

Let $u = \tan(x)$, then $du = \sec^2(x) dx$ or $dx = \frac{du}{\sec^2(x)} = \frac{du}{1+u^2}$

So:
$$\int \frac{2}{1 + \tan(x) + \tan^2(x)} dx = \int \frac{2}{1 + u + u^2} \cdot \frac{du}{1+u^2}$$

This becomes:
$$\int \frac{2}{(1+u^2)(1 + u + u^2)} du$$

We can use partial fractions. First, note that $1 + u + u^2 = \left(u + \frac{1}{2}\right)^2 + \frac{3}{4}$

Let's decompose:
$$\frac{2}{(1+u^2)(1 + u + u^2)} = \frac{A}{1+u^2} + \frac{B(u+\frac{1}{2}) + C}{\left(u + \frac{1}{2}\right)^2 + \frac{3}{4}}$$

After solving for coefficients (which is a bit involved), we get:
$$\frac{2}{(1+u^2)(1 + u + u^2)} = \frac{4}{3} \cdot \frac{1}{1+u^2} - \frac{4}{3} \cdot \frac{u+\frac{1}{2}}{\left(u + \frac{1}{2}\right)^2 + \frac{3}{4}}$$

Now, we integrate:
$$\int \frac{4}{3} \cdot \frac{1}{1+u^2} du - \int \frac{4}{3} \cdot \frac{u+\frac{1}{2}}{\left(u + \frac{1}{2}\right)^2 + \frac{3}{4}} du$$

The first integral is standard: $\int \frac{4}{3} \cdot \frac{1}{1+u^2} du = \frac{4}{3} \arctan(u) + C$

For the second integral, let $v = u + \frac{1}{2}$, which gives:
$$\int \frac{4}{3} \cdot \frac{v}{v^2 + \frac{3}{4}} dv = \frac{4}{3} \cdot \frac{1}{2} \ln\left(v^2 + \frac{3}{4}\right) + C = \frac{2}{3} \ln\left(v^2 + \frac{3}{4}\right) + C$$

Substituting back $v = u + \frac{1}{2}$:
$$\frac{2}{3} \ln\left(\left(u + \frac{1}{2}\right)^2 + \frac{3}{4}\right) + C = \frac{2}{3} \ln(1 + u + u^2) + C$$

So, the third part of our integral is:
$$\int \frac{2}{1 + \tan(x) + \tan^2(x)} dx = \frac{4}{3} \arctan(\tan(x)) - \frac{2}{3} \ln(1 + \tan(x) + \tan^2(x)) + C$$

Since $\arctan(\tan(x)) = x$ for $x \in (-\frac{\pi}{2}, \frac{\pi}{2})$, and our integration bounds are from 0 to $\frac{\pi}{4}$, we have:
$$\int \frac{2}{1 + \tan(x) + \tan^2(x)} dx = \frac{4}{3} x - \frac{2}{3} \ln(1 + \tan(x) + \tan^2(x)) + C$$

## Step 3: Combine and evaluate

Combining all parts:
$$\int\left(2\tan(x) + 1 + \frac{2}{1 + \tan(x) + \tan^2(x)}\right) dx = -2\ln|\cos(x)| + x + \frac{4}{3} x - \frac{2}{3} \ln(1 + \tan(x) + \tan^2(x)) + C$$

Simplifying:
$$\int\left(2\tan(x) + 1 + \frac{2}{1 + \tan(x) + \tan^2(x)}\right) dx = -2\ln|\cos(x)| + \frac{7}{3} x - \f