### Definite Integral Evaluation

We are tasked with evaluating the definite integral:

$$
\int_0^2 \sqrt{x} \cdot \sqrt{2 - x} \cdot \cos\left(\sqrt{x(2 - x)}\right) \, dx
$$

---

### Step 1: Simplify the Integrand

Observe that:

$$
\sqrt{x} \cdot \sqrt{2 - x} = \sqrt{x(2 - x)}
$$

So the integral becomes:

$$
\int_0^2 \sqrt{x(2 - x)} \cdot \cos\left(\sqrt{x(2 - x)}\right) \, dx
$$

Let us denote $ u = \sqrt{x(2 - x)} $. Then the integrand becomes $ u \cos(u) $, and we need to express $ dx $ in terms of $ u $.

---

### Step 2: Change of Variables

Let’s analyze the function $ u = \sqrt{x(2 - x)} $. This function reaches its maximum at $ x = 1 $, where $ u = 1 $, and decreases symmetrically to zero at $ x = 0 $ and $ x = 2 $. This symmetry suggests a substitution that simplifies the integral.

Let’s perform a substitution:

$$
x = 1 + t \Rightarrow dx = dt
$$

Then:

$$
x(2 - x) = (1 + t)(1 - t) = 1 - t^2
\Rightarrow \sqrt{x(2 - x)} = \sqrt{1 - t^2}
$$

So the integral becomes:

$$
\int_{-1}^{1} \sqrt{1 - t^2} \cdot \cos\left(\sqrt{1 - t^2}\right) \, dt
$$

Since the integrand is even, we can simplify further:

$$
2 \int_0^1 \sqrt{1 - t^2} \cdot \cos\left(\sqrt{1 - t^2}\right) \, dt
$$

---

### Step 3: Substitution and Bessel Function Connection

Let’s now make the substitution $ u = \sqrt{1 - t^2} $, which implies $ t = \sqrt{1 - u^2} $, and $ dt = -\frac{u}{\sqrt{1 - u^2}} du $

This leads to:

$$
\int_0^1 \sqrt{1 - t^2} \cdot \cos\left(\sqrt{1 - t^2}\right) \, dt = \int_0^1 u \cos u \cdot \frac{u}{\sqrt{1 - u^2}} \, du = \int_0^1 \frac{u^2 \cos u}{\sqrt{1 - u^2}} \, du
$$

This integral is known to be expressible in terms of **Bessel functions**. Specifically:

$$
\int_0^1 \frac{u^2 \cos u}{\sqrt{1 - u^2}} \, du = \frac{\pi}{2} (J_0(1) - J_1(1))
$$

Therefore, the original integral becomes:

$$
2 \cdot \frac{\pi}{2} (J_0(1) - J_1(1)) = \pi (J_0(1) - J_1(1))
$$

---

### Step 4: Numerical Approximation

Using known values of Bessel functions:

- $ J_0(1) \approx 0.7651976865579666 $
- $ J_1(1) \approx 0.4400505857449336 $

Then:

$$
\pi (J_0(1) - J_1(1)) \approx \pi (0.325147100813033) \approx 1.0214796633
$$

---

### Final Answer

$$
\boxed{
\left\{
  "answer": "\\pi \\left( J_0(1) - J_1(1) \\right)",
  "numerical_answer": "1.0214796633"
\right\}
}
$$