We begin by considering the integral

  I = ∫ₑ^(eᵉ) (log x · log(log x))⁄x dx.

Step 1. Substitution:
Let u = log x. Then, du = (dx⁄x).

Under this substitution, when x = e, then u = 1; and when x = eᵉ, then u = e. The integrand becomes:
  log x = u  and  log(log x) = log u.

Thus, the integral becomes:
  I = ∫₁ᵉ u · log u du.

Step 2. Integration:
We now evaluate J = ∫ u · log u du. Use integration by parts. Let
  v = log u  ⇒ dv = (1/u) du,
  dw = u du  ⇒ w = u²⁄2.

Then by the integration by parts formula:
  J = (u²⁄2) · log u − ∫ (u²⁄2) · (1/u) du
  = (u²·log u)⁄2 − (1/2)∫ u du
  = (u²·log u)⁄2 − (1/2)(u²⁄2)
  = (u²·log u)⁄2 − u²⁄4.

Thus, the antiderivative is F(u) = (u²·log u)/2 − u²/4.

Step 3. Evaluate the Definite Integral:
Now evaluate from u = 1 to u = e:
  F(e) = (e²·log e)/2 − e²/4 = (e²·1)/2 − e²/4 = e²/2 − e²/4 = e²/4,
  F(1) = (1²·log 1)/2 − 1²/4 = 0 − 1/4 = −1/4.

Thus, the value is
  I = F(e) − F(1) = (e²/4) − (−1/4) = (e² + 1)/4.

Step 4. Numerical Approximation:
Using the known approximation e² ≈ 7.38905609893,
  I ≈ (7.38905609893 + 1) / 4 ≈ 8.38905609893 / 4 ≈ 2.09726402473.

The final results can be written as:

Exact answer: (e² + 1)/4  
Numerical approximation: 2.0972640247

{"answer": "\\frac{e^2+1}{4}", "numerical_answer": "2.0972640247"}