Let's compute the definite integral:
\[
I = \int_{-1}^1 \frac{\cos x}{1 + e^{-1/x}} \, dx
\]

**Step 1: Analyze symmetry and substitution**

Let us first attempt the substitution \( x \to -x \):

Let \( u = -x \implies dx = -du \), as \( x \) goes from \(-1\) to \(1\), \( u \) goes from \(1\) to \(-1\):

\[
I = \int_{x=-1}^{x=1} \frac{\cos x}{1 + e^{-1/x}} dx = \int_{u=1}^{u=-1} \frac{\cos(-u)}{1 + e^{-1/(-u)}} (-du)
\]
\[
= \int_{u=-1}^{u=1} \frac{\cos(-u)}{1 + e^{1/u}} du
\]
Recall that \(\cos(-u) = \cos u\):

\[
= \int_{-1}^1 \frac{\cos u}{1 + e^{1/u}} du
\]

Now add the original and reflected expressions for the integral:

\[
2I = \int_{-1}^1 \left( \frac{\cos x}{1 + e^{-1/x}} + \frac{\cos x}{1 + e^{1/x}} \right) dx
\]

Now, combine the fractions:

\[
\frac{1}{1 + e^{-1/x}} + \frac{1}{1 + e^{1/x}} = \frac{(1 + e^{1/x}) + (1 + e^{-1/x})}{(1 + e^{-1/x})(1 + e^{1/x})}
\]
\[
= \frac{2 + e^{1/x} + e^{-1/x}}{(1 + e^{-1/x})(1 + e^{1/x})}
\]

But note:
\[
(1 + e^{-1/x})(1 + e^{1/x}) = (1)(1) + (1)e^{1/x} + e^{-1/x}(1) + e^{-1/x}e^{1/x} = 1 + e^{1/x} + e^{-1/x} + 1 = 2 + e^{1/x} + e^{-1/x}
\]
So they cancel, and the expression simplifies to:

\[
\frac{2 + e^{1/x} + e^{-1/x}}{2 + e^{1/x} + e^{-1/x}} = 1
\]

Thus:
\[
2I = \int_{-1}^1 \cos x \, dx
\]
\[
I = \frac{1}{2} \int_{-1}^1 \cos x \, dx
\]

Now:
\[
\int_{-1}^{1} \cos x \, dx = \sin x \Big|_{-1}^{1} = \sin(1) - \sin(-1) = 2 \sin(1)
\]
So,
\[
I = \frac{1}{2} \times 2 \sin(1) = \sin(1)
\]

**Step 2: Numerical approximation**

\[
\sin(1) \approx 0.8414709848
\]

**Step 3: JSON Output**

```json
{"answer": "\\sin 1", "numerical_answer": "0.8414709848"}
```