To evaluate the definite integral:

$$
\int_0^{1.0} x \ln\left(\frac{1.0 + \sqrt{1.0^2 - x^2}}{x}\right) \mathbf{D}(0.5x) \, dx
$$

we begin by analyzing the integrand. The function $\mathbf{D}(0.5x)$ is not explicitly defined in the problem, which presents a challenge. However, assuming that $\mathbf{D}(0.5x)$ refers to the derivative of $0.5x$ with respect to $x$, we have:

$$
\mathbf{D}(0.5x) = \frac{d}{dx}(0.5x) = 0.5
$$

This simplifies the integrand to:

$$
0.5 \cdot x \ln\left(\frac{1.0 + \sqrt{1.0^2 - x^2}}{x}\right)
$$

So the integral becomes:

$$
I = 0.5 \int_0^1 x \ln\left(\frac{1 + \sqrt{1 - x^2}}{x}\right) dx
$$

---

### Step 1: Simplify the Logarithmic Expression

We simplify the logarithmic term:

$$
\ln\left(\frac{1 + \sqrt{1 - x^2}}{x}\right) = \ln(1 + \sqrt{1 - x^2}) - \ln x
$$

So the integral becomes:

$$
I = 0.5 \left[ \int_0^1 x \ln(1 + \sqrt{1 - x^2}) \, dx - \int_0^1 x \ln x \, dx \right]
$$

---

### Step 2: Evaluate Each Integral Separately

#### Integral A: $\int_0^1 x \ln x \, dx$

This is a standard integral:

$$
\int_0^1 x \ln x \, dx = -\frac{1}{4}
$$

#### Integral B: $\int_0^1 x \ln(1 + \sqrt{1 - x^2}) \, dx$

We use the substitution $ u = 1 - x^2 $, $ du = -2x dx $, which transforms the integral into:

$$
\int_0^1 x \ln(1 + \sqrt{1 - x^2}) \, dx = 0.5 \int_0^1 \ln(1 + \sqrt{u}) \, du
$$

Now, substitute $ t = \sqrt{u} $, $ u = t^2 $, $ du = 2t dt $, and the integral becomes:

$$
\int_0^1 \ln(1 + t) \cdot 2t \, dt
$$

This is evaluated via integration by parts:

$$
\int_0^1 2t \ln(1 + t) \, dt = \left[ t^2 \ln(1 + t) \right]_0^1 - \int_0^1 \frac{t^2}{1 + t} \, dt
$$

The boundary term is:

$$
[1^2 \ln 2 - 0] = \ln 2
$$

The remaining integral simplifies:

$$
\int_0^1 \frac{t^2}{1 + t} \, dt = \int_0^1 \left( t - 1 + \frac{1}{1 + t} \right) dt = \left[ \frac{t^2}{2} - t + \ln(1 + t) \right]_0^1 = -\frac{1}{2} + \ln 2
$$

So the integral becomes:

$$
\ln 2 - (-\frac{1}{2} + \ln 2) = \frac{1}{2}
$$

Thus:

$$
\int_0^1 x \ln(1 + \sqrt{1 - x^2}) \, dx = 0.5 \cdot \frac{1}{2} = \frac{1}{4}
$$

---

### Step 3: Combine the Results

Now we combine the two integrals:

$$
I = 0.5 \left[ \frac{1}{4} - \left(-\frac{1}{4}\right) \right] = 0.5 \left( \frac{1}{4} + \frac{1}{4} \right) = 0.5 \