We wish to evaluate

  I = ∫₀² x^(–1/2) · H₃( x(2 – x)^(1/4) ) dx

where H₃ is the third Hermite polynomial. In the “physicists’” convention the Hermite polynomials are given by

  H₃(z) = 8z³ – 12z.

Thus, with z = (x(2 – x))^(1/4), we have
  H₃( (x(2 – x))^(1/4) ) = 8 [x(2 – x)]^(3/4) – 12 [x(2 – x)]^(1/4).

Then the integrand becomes

  x^(–1/2) [8 (x(2 – x))^(3/4) – 12 (x(2 – x))^(1/4)]
    = 8 x^(–1/2) x^(3/4) (2 – x)^(3/4) – 12 x^(–1/2) x^(1/4) (2 – x)^(1/4)
    = 8 x^(1/4) (2 – x)^(3/4) – 12 x^(–1/4) (2 – x)^(1/4).

Thus our integral is

  I = ∫₀² [8 x^(1/4)(2 – x)^(3/4) – 12 x^(–1/4)(2 – x)^(1/4)] dx.

Step 1. Change of variable

Let
  x = 2u, dx = 2 du.
When x goes from 0 to 2, u goes from 0 to 1. Also note that
  2 – x = 2 – 2u = 2(1 – u).

Substitute into the integrals:

The first term becomes:
  8 (2u)^(1/4)[2(1 – u)]^(3/4) = 8 · 2^(1/4) u^(1/4) · 2^(3/4)(1 – u)^(3/4)
    = 8 · 2^(1/4+3/4) u^(1/4)(1 – u)^(3/4) = 8 · 2 u^(1/4)(1 – u)^(3/4) = 16 u^(1/4)(1 – u)^(3/4).

The second term becomes:
  12 (2u)^(–1/4)[2(1 – u)]^(1/4) = 12 · 2^(–1/4) u^(–1/4) · 2^(1/4)(1 – u)^(1/4)
    = 12 u^(–1/4)(1 – u)^(1/4).

Also, dx = 2 du so the whole integral becomes

  I = 2 ∫₀¹ { 16 u^(1/4)(1 – u)^(3/4) – 12 u^(–1/4)(1 – u)^(1/4) } du
    = 32 ∫₀¹ u^(1/4)(1 – u)^(3/4) du – 24 ∫₀¹ u^(–1/4)(1 – u)^(1/4) du.

Step 2. Express in terms of the Beta function

Recall that the Beta function is defined as

  B(a, b) = ∫₀¹ u^(a–1) (1 – u)^(b–1) du = Γ(a)Γ(b)/Γ(a+b).

For the first integral we note:
  u^(1/4) = u^((5/4) – 1) and (1 – u)^(3/4) = (1 – u)^((7/4) – 1).
Thus, with a = 5/4 and b = 7/4,
  ∫₀¹ u^(1/4)(1 – u)^(3/4) du = B(5/4, 7/4) = Γ(5/4)Γ(7/4)/Γ(3).

Since Γ(3) = 2, the first term is
  32 · B(5/4, 7/4) = 32 (Γ(5/4)Γ(7/4))/2 = 16 Γ(5/4)Γ(7/4).

For the second integral, write:
  u^(–1/4) = u^((3/4) – 1) and (1 – u)^(1/4) = (1 – u)^((5/4) – 1).
Thus, with a = 3/4 and b = 5/4,
  ∫₀¹ u^(–1/4)(1 – u)^(1/4) du = B(3/4, 5/4) = Γ(3/4)Γ(5/4)/Γ(2).

Since Γ(2) = 1,
  the second term is
  24 · B(3/4, 5/4) = 24 Γ(3/4)Γ(5/4).

Thus, our integral becomes

  I = 16 Γ(5/4)Γ(7/4) – 24 Γ(3/4)Γ(5/4).

We may factor out the common factor Γ(5/4):

  I = Γ(5/4)[16 Γ(7/4) – 24 Γ(3/4)]
    = 8 Γ(5/4)[2 Γ(7/4) – 3 Γ(3/4)].

Step 3. Use the Gamma recurrence

Recall that for any z, Γ(z+1) = zΓ(z). With z = 3/4, we have

  Γ(7/4) = (3/4) Γ(3/4).

Substitute this into the expression:

  2 Γ(7/4) – 3 Γ(3/4) = 2·(3/4)Γ(3/4) – 3Γ(3/4) = (3/2 – 3) Γ(3/4) = –(3/2)Γ(3/4).

Thus, the integral becomes

  I = 8 Γ(5/4) [ –(3/2) Γ(3/4) ] = –12 Γ(5/4)Γ(3/4).

Step 4. Express the Gamma product in closed‐form

There is a well-known identity relating Γ(1/4) and Γ(3/4):

  Γ(1/4)Γ(3/4) = π√2.

Also note that
  Γ(5/4) = (1/4) Γ(1/4),   (since Γ(z+1) = z Γ(z) with z = 1/4).

Thus, we have

  Γ(5/4)Γ(3/4) = (1/4) Γ(1/4)Γ(3/4) = (1/4)(π√2) = (π√2)/4.

Substitute back in:

  I = –12 · (π√2)/4 = –3π√2.

Step 5. Numerical approximation

We now approximate
  I = –3π√2.
With
  π ≈ 3.141592653589793 and √2 ≈ 1.414213562373095,
we get

  π√2 ≈ 3.141592653589793 × 1.414213562373095 ≈ 4.442882938158366,
  I ≈ –3 × 4.442882938158366 ≈ –13.328648814475098.

Rounded to 10 decimal places, the numerical approximation is –13.3286488145.

Final Answer in JSON Format:
{"answer": "$-3\\pi\\sqrt{2}$", "numerical_answer": "-13.3286488145"}