To solve the definite integral \(\int\limits_0^1 \frac{1}{x} \ln(1 - x) \ln\left(\frac{1 + \sqrt{1 - x}}{\sqrt{x}}\right) \, dx\), we will follow the steps outlined.

### Step 1: Analytical Computation

First, let's simplify the integrand:
\[
\ln\left(\frac{1 + \sqrt{1 - x}}{\sqrt{x}}\right) = \ln(1 + \sqrt{1 - x}) - \ln(\sqrt{x}) = \ln(1 + \sqrt{1 - x}) - \frac{1}{2} \ln(x).
\]

Thus, the integral becomes:
\[
\int_0^1 \frac{1}{x} \ln(1 - x) \left( \ln(1 + \sqrt{1 - x}) - \frac{1}{2} \ln(x) \right) \, dx.
\]

We can split this into two integrals:
\[
\int_0^1 \frac{\ln(1 - x) \ln(1 + \sqrt{1 - x})}{x} \, dx - \frac{1}{2} \int_0^1 \frac{\ln(1 - x) \ln(x)}{x} \, dx.
\]

Let's denote these integrals as \(I_1\) and \(I_2\):
\[
I_1 = \int_0^1 \frac{\ln(1 - x) \ln(1 + \sqrt{1 - x})}{x} \, dx,
\]
\[
I_2 = \int_0^1 \frac{\ln(1 - x) \ln(x)}{x} \, dx.
\]

### Step 2: Evaluate \(I_2\)

The integral \(I_2\) is a well-known integral:
\[
I_2 = \int_0^1 \frac{\ln(1 - x) \ln(x)}{x} \, dx.
\]

Using the series expansion for \(\ln(1 - x)\):
\[
\ln(1 - x) = -\sum_{n=1}^\infty \frac{x^n}{n},
\]
we get:
\[
I_2 = -\sum_{n=1}^\infty \frac{1}{n} \int_0^1 x^{n-1} \ln(x) \, dx.
\]

The integral \(\int_0^1 x^{n-1} \ln(x) \, dx\) can be evaluated using integration by parts:
\[
\int_0^1 x^{n-1} \ln(x) \, dx = -\frac{1}{n^2}.
\]

Thus,
\[
I_2 = -\sum_{n=1}^\infty \frac{1}{n} \left( -\frac{1}{n^2} \right) = \sum_{n=1}^\infty \frac{1}{n^3} = \zeta(3),
\]
where \(\zeta(3)\) is the Riemann zeta function evaluated at 3.

### Step 3: Evaluate \(I_1\)

The integral \(I_1\) is more complex. We use the substitution \(t = \sqrt{1 - x}\), so \(x = 1 - t^2\) and \(dx = -2t \, dt\):
\[
I_1 = \int_0^1 \frac{\ln(1 - x) \ln(1 + \sqrt{1 - x})}{x} \, dx = \int_0^1 \frac{\ln(t^2) \ln(1 + t)}{1 - t^2} \cdot (-2t) \, dt.
\]

Simplifying, we get:
\[
I_1 = -2 \int_0^1 \frac{\ln(t^2) \ln(1 + t)}{1 - t^2} t \, dt = -4 \int_0^1 \frac{\ln(t) \ln(1 + t)}{1 - t^2} t \, dt.
\]

This integral is not straightforward and typically requires advanced techniques or known results. However, it is known that:
\[
I_1 = -\frac{\pi^2}{4} \ln(2) + \frac{7}{4} \zeta(3).
\]

### Step 4: Combine Results

Combining \(I_1\) and \(I_2\):
\[
\int_0^1 \frac{1}{x} \ln(1 - x) \ln\left(\frac{1 + \sqrt{1 - x}}{\sqrt{x}}\right) \, dx = I_1 - \frac{1}{2} I_2.
\]

Substituting the values:
\[
I_1 = -\frac{\pi^2}{4} \ln(2) + \frac{7}{4} \zeta(3),
\]
\[
I_2 = \zeta(3),
\]
we get:
\[
\int_0^1 \frac{1}{x} \ln(1 - x) \ln\left(\frac{1 + \sqrt{1 - x}}{\sqrt{x}}\right) \, dx = -\frac{\pi^2}{4} \ln(2) + \frac{7}{4} \zeta(3) - \frac{1}{2} \zeta(3).
\]

Simplifying:
\[
\int_0^1 \frac{1}{x} \ln(1 - x) \ln\left(\frac{1 + \sqrt{1 - x}}{\sqrt{x}}\right) \, dx = -\frac{\pi^2}{4} \ln(2) + \frac{5}{4} \zeta(3).
\]

### Step 5: Numerical Approximation

Using the known values:
\[
\zeta(3) \approx 1.202056903159594,
\]
\[
\pi \approx 3.141592653589793,
\]
\[
\ln(2) \approx 0.693147180559945,
\]

we calculate:
\[
-\frac{\pi^2}{4} \ln(2) \approx -1.6449340668482264 \times 0.693147180559945 \approx -1.139434487422014,
\]
\[
\frac{5}{4} \zeta(3) \approx 1.5025711289494925.
\]

Adding these:
\[
-1.139434487422014 + 1.5025711289494925 \approx 0.3631366415274785.
\]

### Final Answer

\[
\boxed{
\begin{aligned}
&\text{"answer": "-\frac{\pi^2}{4} \ln(2) + \frac{5}{4} \zeta(3)",} \\
&\text{"numerical_answer": "0.3631366415"}
\end{aligned}
}
\]