To solve the given definite integral:

\[
\int_{0}^{2.0} x^{-1/2} (2.0 - x)^{-1/2} (1 + 0.5x)^{-1 - 1} T_{2 \times 1}\left(\sqrt{1 + 0.5x}\right) \, dx,
\]

let's break it down step by step.

### Step 1: Simplify the Integrand
First, rewrite the integrand in a more manageable form:

1. **Exponents and Coefficients**:
   - \( x^{-1/2} = \frac{1}{\sqrt{x}} \)
   - \( (2.0 - x)^{-1/2} = \frac{1}{\sqrt{2 - x}} \)
   - \( (1 + 0.5x)^{-1 - 1} = (1 + 0.5x)^{-2} = \frac{1}{(1 + 0.5x)^2} \)

2. **Chebyshev Polynomial \( T_{2 \times 1} \)**:
   - \( T_{2 \times 1}(y) = T_2(y) \), where \( T_2(y) = 2y^2 - 1 \).
   - Here, \( y = \sqrt{1 + 0.5x} \), so:
     \[
     T_2\left(\sqrt{1 + 0.5x}\right) = 2(1 + 0.5x) - 1 = 1 + x
     \]

Now, substitute \( T_2 \) back into the integrand:
\[
\frac{1}{\sqrt{x}} \cdot \frac{1}{\sqrt{2 - x}} \cdot \frac{1}{(1 + 0.5x)^2} \cdot (1 + x)
\]

### Step 2: Combine Terms
The integrand becomes:
\[
\frac{1 + x}{\sqrt{x} \sqrt{2 - x} (1 + 0.5x)^2}
\]

### Step 3: Variable Substitution
Let \( x = 2 \sin^2 \theta \), which implies:
- \( dx = 4 \sin \theta \cos \theta \, d\theta \)
- When \( x = 0 \), \( \theta = 0 \)
- When \( x = 2 \), \( \theta = \frac{\pi}{2} \)

Substitute \( x \) and \( dx \):
\[
\sqrt{x} = \sqrt{2} \sin \theta, \quad \sqrt{2 - x} = \sqrt{2} \cos \theta, \quad 1 + 0.5x = 1 + \sin^2 \theta
\]

The integrand becomes:
\[
\frac{1 + 2 \sin^2 \theta}{\sqrt{2} \sin \theta \cdot \sqrt{2} \cos \theta \cdot (1 + \sin^2 \theta)^2} \cdot 4 \sin \theta \cos \theta \, d\theta
\]

Simplify:
\[
\frac{(1 + 2 \sin^2 \theta) \cdot 4 \sin \theta \cos \theta}{2 \sin \theta \cos \theta \cdot (1 + \sin^2 \theta)^2} = \frac{2 (1 + 2 \sin^2 \theta)}{(1 + \sin^2 \theta)^2} \, d\theta
\]

### Step 4: Simplify the Integral
The integral now is:
\[
2 \int_{0}^{\pi/2} \frac{1 + 2 \sin^2 \theta}{(1 + \sin^2 \theta)^2} \, d\theta
\]

Let \( u = \sin^2 \theta \), but this substitution is not straightforward. Instead, use the identity \( \sin^2 \theta = \frac{1 - \cos 2\theta}{2} \):
\[
1 + \sin^2 \theta = 1 + \frac{1 - \cos 2\theta}{2} = \frac{3 - \cos 2\theta}{2}
\]
\[
1 + 2 \sin^2 \theta = 1 + (1 - \cos 2\theta) = 2 - \cos 2\theta
\]

The integral becomes:
\[
2 \int_{0}^{\pi/2} \frac{2 - \cos 2\theta}{\left(\frac{3 - \cos 2\theta}{2}\right)^2} \, d\theta = 8 \int_{0}^{\pi/2} \frac{2 - \cos 2\theta}{(3 - \cos 2\theta)^2} \, d\theta
\]

### Step 5: Further Simplification
Let \( \phi = 2\theta \), \( d\phi = 2 d\theta \), bounds remain \( 0 \) to \( \pi \):
\[
8 \cdot \frac{1}{2} \int_{0}^{\pi} \frac{2 - \cos \phi}{(3 - \cos \phi)^2} \, d\phi = 4 \int_{0}^{\pi} \frac{2 - \cos \phi}{(3 - \cos \phi)^2} \, d\phi
\]

This integral can be evaluated using residue calculus or known integral tables. The result is:
\[
4 \cdot \frac{\pi}{2 \sqrt{2}} = \pi \sqrt{2}
\]

### Step 6: Numerical Approximation
The exact answer is \( \pi \sqrt{2} \). Numerically:
\[
\pi \sqrt{2} \approx 4.4428829381
\]

### Final Answer
```json
{"answer": "\\pi \\sqrt{2}", "numerical_answer": "4.4428829381"}
```