To evaluate the definite integral  
$$
\int_0^1 \sqrt[4]{\frac{1}{x} - 1} \, dx,
$$  
we begin by simplifying the integrand. Observe that:
$$
\frac{1}{x} - 1 = \frac{1 - x}{x},
$$
so the integrand becomes:
$$
\left( \frac{1 - x}{x} \right)^{1/4}.
$$
Thus, the integral becomes:
$$
\int_0^1 \left( \frac{1 - x}{x} \right)^{1/4} dx.
$$

---

### Step 1: Substitution

Let us make the substitution:
$$
t = \left( \frac{1 - x}{x} \right)^{1/4}.
$$
Raising both sides to the 4th power gives:
$$
t^4 = \frac{1 - x}{x} \quad \Rightarrow \quad x = \frac{1}{t^4 + 1}.
$$
Differentiating both sides with respect to $ t $, we get:
$$
dx = -\frac{4t^3}{(t^4 + 1)^2} dt.
$$

Now, we adjust the limits of integration:
- When $ x \to 0^+ $, $ t \to \infty $,
- When $ x = 1 $, $ t = 0 $.

Reversing the limits to eliminate the negative sign, the integral becomes:
$$
\int_0^\infty \frac{4t^4}{(t^4 + 1)^2} dt.
$$

---

### Step 2: Recognizing the Beta Function Form

We now recognize that this integral is in the form of a standard Beta function. Let us perform the substitution:
$$
u = t^4 \quad \Rightarrow \quad t = u^{1/4}, \quad dt = \frac{1}{4} u^{-3/4} du.
$$
Substituting into the integral:
$$
\int_0^\infty \frac{4t^4}{(t^4 + 1)^2} dt = \int_0^\infty \frac{4u}{(u + 1)^2} \cdot \frac{1}{4} u^{-3/4} du = \int_0^\infty \frac{u^{1/4}}{(u + 1)^2} du.
$$

This is now in the standard Beta function form:
$$
\int_0^\infty \frac{u^{a - 1}}{(1 + u)^{a + b}} du = B(a, b),
$$
where $ a = \frac{5}{4} $ and $ b = \frac{3}{4} $. Thus:
$$
\int_0^\infty \frac{u^{1/4}}{(u + 1)^2} du = B\left( \frac{5}{4}, \frac{3}{4} \right).
$$

Using the identity $ B(a, b) = \frac{\Gamma(a)\Gamma(b)}{\Gamma(a + b)} $, we have:
$$
B\left( \frac{5}{4}, \frac{3}{4} \right) = \frac{\Gamma\left( \frac{5}{4} \right)\Gamma\left( \frac{3}{4} \right)}{\Gamma(2)}.
$$
Since $ \Gamma(2) = 1! = 1 $, and using the identity:
$$
\Gamma\left( \frac{5}{4} \right) = \frac{1}{4} \Gamma\left( \frac{1}{4} \right),
$$
we get:
$$
\Gamma\left( \frac{5}{4} \right)\Gamma\left( \frac{3}{4} \right) = \frac{1}{4} \Gamma\left( \frac{1}{4} \right)\Gamma\left( \frac{3}{4} \right).
$$

Now, applying the reflection formula:
$$
\Gamma(z)\Gamma(1 - z) = \frac{\pi}{\sin(\pi z)},
$$
with $ z = \frac{1}{4} $, we find:
$$
\Gamma\left( \frac{1}{4} \right)\Gamma\left( \frac{3}{4} \right) = \frac{\pi}{\sin\left( \frac{\pi}{4} \right)} =