

To calculate the definite integral \( \int_{-1}^1 \frac{1}{3^x + 1} \, dx \), we use a substitution technique to simplify the integrand.

### Step 1: Define the integral and substitute \( x \to -x \)
Let \( I = \int_{-1}^1 \frac{1}{3^x + 1} \, dx \). Consider the substitution \( u = -x \), which implies \( du = -dx \). When \( x = -1 \), \( u = 1 \), and when \( x = 1 \), \( u = -1 \). Rewriting the integral in terms of \( u \):
\[
I = \int_{1}^{-1} \frac{1}{3^{-u} + 1} (-du) = \int_{-1}^1 \frac{1}{3^{-u} + 1} \, du.
\]
Since the variable of integration is a dummy variable, we replace \( u \) with \( x \):
\[
I = \int_{-1}^1 \frac{1}{3^{-x} + 1} \, dx.
\]

### Step 2: Simplify the substituted integrand
Note that \( 3^{-x} = \frac{1}{3^x} \), so:
\[
\frac{1}{3^{-x} + 1} = \frac{1}{\frac{1}{3^x} + 1} = \frac{3^x}{1 + 3^x}.
\]
Thus, the integral becomes:
\[
I = \int_{-1}^1 \frac{3^x}{3^x + 1} \, dx.
\]

### Step 3: Add the original and substituted integrals
Adding the original integral \( I \) and the substituted integral \( I \):
\[
2I = \int_{-1}^1 \left( \frac{1}{3^x + 1} + \frac{3^x}{3^x + 1} \right) dx.
\]
The integrand simplifies to:
\[
\frac{1 + 3^x}{3^x + 1} = 1.
\]
Thus:
\[
2I = \int_{-1}^1 1 \, dx = \left[ x \right]_{-1}^1 = 1 - (-1) = 2.
\]
Solving for \( I \), we get \( I = 1 \).

### Numerical Approximation
The exact value is \( 1 \), so the numerical approximation is \( 1.0000000000 \).

{"answer": "1", "numerical_answer": "1.0000000000"}