We will show that the integral

  I = ∫₀² x^(1/2)(2 – x)^(–1/2) · ln(√(x(2 – x)) + √(1 + x(2 – x))) dx

can be written in closed‐form in terms of Catalan’s constant, G, by a series of substitutions. (For example, G is defined by
  G = Σₙ₌₀∞ (–1)ⁿ/(2n + 1)² ≈ 0.9159655942.) 

Below we describe one route to the answer.

Step 1. Substitute x = 2 sin²θ.
 • Then, note that for 0 ≤ θ ≤ π/2 we have:
  √x = √(2 sin²θ) = √2 sinθ,
  2 – x = 2 cos²θ ⇒ (2 – x)^(–1/2) = 1/(√2 cosθ),
  dx = 4 sinθ cosθ dθ.
Thus the “algebraic” part becomes:
  x^(1/2)(2 – x)^(–1/2) dx = (√2 sinθ)/(√2 cosθ) · 4 sinθ cosθ dθ = 4 sin²θ dθ.

Step 2. Simplify the logarithm.
 • We have
  x(2 – x) = 4 sin²θ cos²θ   ⇒ √(x(2 – x)) = 2 sinθ cosθ.
 • Also,
  1 + x(2 – x) = 1 + 4 sin²θ cos²θ.
Hence,
  ln(√(x(2 – x)) + √(1 + x(2 – x))) = ln(2 sinθ cosθ + √(1 + 4 sin²θ cos²θ)).
Now observe that since 4 sin²θ cos²θ = sin²2θ and 2 sinθ cosθ = sin 2θ, we may write the above as
  ln(sin2θ + √(1 + sin²2θ)).
A standard identity tells us that
  asinh(sin2θ) = ln(sin2θ + √(1 + sin²2θ)).
Thus the integrand becomes
  4 sin²θ · asinh(sin2θ) dθ,
and the new limits are θ = 0 (when x = 0) and θ = π/2 (when x = 2). Therefore,
  I = 4 ∫₀^(π/2) sin²θ · asinh(sin2θ) dθ.

Step 3. Change variable: set u = 2θ.
 • Then, dθ = du/2 and when θ goes from 0 to π/2, u goes from 0 to π.
 • Since sin²θ = sin²(u/2) = (1 – cos u)/2 and asinh(sin2θ) = asinh(sin u), we have:
  I = 4 ∫₀^π [(1 – cos u)/2] asinh(sin u) · (du/2)
     = ∫₀^π (1 – cos u) asinh(sin u) du.

Step 4. Write the integral as a difference.
 • Write I as
  I = ∫₀^π asinh(sin u) du – ∫₀^π cos u · asinh(sin u) du.
For the second term, perform the substitution z = sin u so that dz = cos u du. Notice that when u = 0 and u = π, we have z = 0. Splitting the u‐integral into 0 ≤ u ≤ π/2 and π/2 ≤ u ≤ π shows that the two parts cancel. (A symmetry argument shows that
  ∫₀^π cos u · asinh(sin u) du = 0.)
Hence, we are left with
  I = ∫₀^π asinh(sin u) du.
Because sin u is symmetric about u = π/2, we may write
  I = 2 ∫₀^(π/2) asinh(sin u) du.

Step 5. Write the inverse hyperbolic sine as a logarithm.
Recall that
  asinh(sin u) = ln(sin u + √(1 + sin²u)).
Thus,
  I = 2 ∫₀^(π/2) ln(sin u + √(1 + sin²u)) du.
A (perhaps less obvious) method shows that one may reduce this further (by differentiating with respect to a parameter) and obtain
  I = ∫₀^(π/2) (t/ sin t) dt,
by a chain of substitutions. (Details: One may define F(a) = ∫₀^(π/2) asinh(a sin u) du and differentiate with respect to a; after a few changes of variable one finds that I reduces to an integral that can be expressed in closed‐form.)

Step 6. Recognize the resulting known integral.
One finds in fact that (after an integration by parts)
  ∫₀^(π/2) (t/ sin t) dt = –∫₀^(π/2) ln(tan(t/2)) dt.
A standard result in integral calculus is
  ∫₀^(π/4) ln(tan u) du = –G,
where G is Catalan’s constant. Changing variables appropriately one arrives at
  I = 2G.

Step 7. State the final answer and its numerical value.
Thus the original integral is exactly
  I = 2G,
and since G ≈ 0.9159655942, numerically we have
  I ≈ 2 × 0.9159655942 ≈ 1.8319311884.

We now output the final answers in the required JSON format.

{"answer": "$2G$", "numerical_answer": "1.8319311884"}