Let's solve the definite integral:
\[
I = \int_0^1 x \arcsin x \arccos x \, dx
\]

### Step 1: Simplifying the Integrand

Recall that \( \arcsin x + \arccos x = \frac{\pi}{2} \), so \( \arccos x = \frac{\pi}{2} - \arcsin x \):

\[
I = \int_0^1 x \arcsin x \left( \frac{\pi}{2} - \arcsin x \right) dx = \frac{\pi}{2} \int_0^1 x \arcsin x \, dx - \int_0^1 x (\arcsin x)^2\, dx
\]

Let's call:

\[
I_1 = \int_0^1 x \arcsin x \, dx
\]
\[
I_2 = \int_0^1 x (\arcsin x)^2 \, dx
\]

So,
\[
I = \frac{\pi}{2} I_1 - I_2
\]

--

### Step 2: Compute \( I_1 \)

Use integration by parts:

Let \( u = \arcsin x \implies du = \frac{1}{\sqrt{1-x^2}}dx \)
Let \( dv = x dx \implies v = \frac{1}{2} x^2 \)

So,
\[
I_1 = \int x \arcsin x\, dx = \arcsin x \cdot \frac{1}{2} x^2 - \int \frac{1}{2} x^2 \cdot \frac{1}{\sqrt{1-x^2}}dx
\]

Let’s compute the indefinite integral:

\[
\int x \arcsin x \, dx = \frac{1}{2} x^2 \arcsin x - \frac{1}{2} \int \frac{x^2}{\sqrt{1-x^2}} dx 
\]

Let’s focus on \(\int \frac{x^2}{\sqrt{1-x^2}} dx\).

Recall:
\[
x^2 = 1 - (1 - x^2)
\]
So,
\[
\frac{x^2}{\sqrt{1-x^2}} = \frac{1}{\sqrt{1-x^2}} - \frac{1-x^2}{\sqrt{1-x^2}} = \frac{1}{\sqrt{1-x^2}} - \sqrt{1-x^2}
\]

Therefore,

\[
I_1 = \frac{1}{2} x^2 \arcsin x - \frac{1}{2} \int \left[ \frac{1}{\sqrt{1-x^2}} - \sqrt{1-x^2} \right] dx
\]

Integrate:

- \( \int \frac{1}{\sqrt{1-x^2}} dx = \arcsin x \)
- \( \int \sqrt{1-x^2} dx = \frac{1}{2} (x \sqrt{1-x^2} + \arcsin x) \)

So,

\[
I_1 = \frac{1}{2} x^2 \arcsin x 
- \frac{1}{2} \arcsin x 
+ \frac{1}{4} (x \sqrt{1-x^2} + \arcsin x )
\]

Simplify:

\[
I_1 = \frac{1}{2} x^2 \arcsin x - \frac{1}{4} \arcsin x + \frac{1}{4} x \sqrt{1-x^2}
\]

Evaluate from 0 to 1:

At \( x = 1: \arcsin 1 = \frac{\pi}{2}, \sqrt{1 - 1^2} = 0 \)
At \( x = 0: \arcsin 0 = 0, \sqrt{1-0} = 1 \)

So,

\[
I_1 = \left[ \frac{1}{2}(1)^2 \frac{\pi}{2} - \frac{1}{4}\frac{\pi}{2} + \frac{1}{4}(1)(0)\right]
- \left[0 - 0 + \frac{1}{4} \cdot 0\right]
\]

\[
= \frac{\pi}{4} - \frac{\pi}{8}
= \frac{\pi}{8}
\]

--

### Step 3: Compute \( I_2 = \int_0^1 x (\arcsin x)^2 dx \)

Use integration by parts:

Let \( u = (\arcsin x)^2 \implies du = 2 \arcsin x \frac{1}{\sqrt{1-x^2}}dx \)
Let \( dv = x dx \implies v = \frac{1}{2} x^2 \)

Then,

\[
I_2 = \int x (\arcsin x)^2 dx = \frac{1}{2} x^2 (\arcsin x)^2 - \int \frac{1}{2} x^2 \cdot 2 \arcsin x \frac{1}{\sqrt{1-x^2}} dx
= \frac{1}{2} x^2 (\arcsin x)^2 - \int x^2 \frac{\arcsin x}{\sqrt{1-x^2}} dx
\]

So define:

\[
J = \int x^2 \frac{\arcsin x}{\sqrt{1-x^2}} dx
\]

Recall from earlier:

\[
x^2 = 1 - (1-x^2)
\implies x^2 \frac{\arcsin x}{\sqrt{1-x^2}} = \frac{\arcsin x}{\sqrt{1-x^2}} - \arcsin x \sqrt{1-x^2}
\]

Therefore,
\[
J = \int \left( \frac{\arcsin x}{\sqrt{1-x^2}} - \arcsin x \sqrt{1-x^2} \right) dx
\]

Let’s integrate term-by-term.

- \( \int \frac{\arcsin x}{\sqrt{1-x^2}} dx \):

Let \( t = \arcsin x \implies x = \sin t, dx = \cos t dt \)
\( \sqrt{1-x^2} = \sqrt{1-\sin^2 t} = \cos t \)
So:

\[
\int \frac{t}{\cos t} \cos t dt = \int t dt = \frac{1}{2} t^2 = \frac{1}{2} (\arcsin x)^2
\]

- \( \int \arcsin x \sqrt{1-x^2} dx \):

Again with \( x = \sin t, dx = \cos t dt \), \( \arcsin x = t \), \( \sqrt{1-x^2} = \cos t \):

\[
\int t \cos t dx = \int t \cos t \cos t dt = \int t \cos^2 t dt
\]
But \( dx = \cos t dt \), so:

\[
\int t \cos t dx = \int t \cos t \cos t dt = \int t \cos^2 t dt
\]
But for our integrand, it's \( \arcsin x \sqrt{1-x^2} dx \), or \( t \cos t dt \):

So,

\[
\int t \cos t dt
\]

Integrate by parts:

Let \( a = t \implies da = dt \),
\( db = \cos t dt \implies b = \sin t \).

So,

\[
\int t \cos t dt = t \sin t - \int \sin t dt = t \sin t + \cos t + C
\]

Substituting back:

\[
\int \arcsin x \sqrt{1-x^2} dx = \arcsin x \cdot x + \sqrt{1-x^2}
\]

Thus, collect all this:

\[
J = \int \frac{\arcsin x}{\sqrt{1-x^2}} dx - \int \arcsin x \sqrt{1-x^2} dx
= \frac{1}{2} (\arcsin x)^2 - (\arcsin x \cdot x + \sqrt{1-x^2} )
\]

So,

\[
I_2 = \frac{1}{2} x^2 (\arcsin x)^2 - \left[ \frac{1}{2} (\arcsin x)^2 - x \arcsin x - \sqrt{1-x^2} \right]
\]
\[
= \frac{1}{2} x^2 (\arcsin x)^2 - \frac{1}{2} (\arcsin x)^2 + x \arcsin x + \sqrt{1-x^2}
\]

Now, evaluate from 0 to 1:

At \( x = 1 \):

- \( x^2 = 1 \)
- \( \arcsin 1 = \frac{\pi}{2} \)
- \( \sqrt{1-1^2} = 0 \)

So,

- \( \frac{1}{2} x^2 (\arcsin x)^2 \) at 1: \( \frac{1}{2} \cdot 1 \cdot (\frac{\pi}{2})^2 = \frac{1}{2} \cdot \frac{\pi^2}{4} = \frac{\pi^2}{8} \)
- \( -\frac{1}{2} (\arcsin x)^2 \) at 1: \( -\frac{1}{2} \cdot \frac{\pi^2}{4} = -\frac{\pi^2}{8} \)
- \( x \arcsin x \) at 1: \( 1 \cdot \frac{\pi}{2} = \frac{\pi}{2} \)
- \( \sqrt{1 - x^2} \) at 1: 0

So sum at x=1:

\[
\frac{\pi^2}{8} - \frac{\pi^2}{8} + \frac{\pi}{2} + 0 = \frac{\pi}{2}
\]

At \( x = 0 \):

- \( x^2 = 0 \)
- \( \arcsin 0 = 0 \)
- \( x \arcsin 0 = 0 \)
- \( \sqrt{1-0^2} = 1 \)

So:

\[
0 - 0 + 0 + 1 = 1
\]

Now, the definite integral:

\[
I_2 = \left( \frac{\pi}{2} \right) - 1
\]

--

### Step 4: Put it all together

Recall:

\[
I = \frac{\pi}{2} I_1 - I_2 = \frac{\pi}{2} \cdot \frac{\pi}{8} - \left( \frac{\pi}{2} - 1 \right) = \frac{\pi^2}{16} - \frac{\pi}{2} + 1
\]

---

### Step 5: Decimal Approximation

Let’s compute the decimal value up to 10 decimal places:

- \( \pi \approx 3.1415926536 \)
- \( \pi^2 \approx 9.8696044011 \)
- \( \frac{\pi^2}{16} \approx 0.6168502751 \)
- \( \frac{\pi}{2} \approx 1.5707963268 \)

Therefore,
\[
I \approx 0.6168502751 - 1.5707963268 + 1 = 0.0460539483
\]

---

### Step 6: Final Answer (JSON FORMAT)

```json
{"answer": "\\frac{\\pi^2}{16} - \\frac{\\pi}{2} + 1", "numerical_answer": "0.0460539483"}
```