Let's solve the definite integral:
\[
\int_{0}^{1} \frac{x^3 + x + 1}{3x^2 - 3x + 4} \, dx
\]

**Step 1: Simplify the numerator.**

Divide \( x^3 + x + 1 \) by the quadratic denominator \( 3x^2 - 3x + 4 \) to see if we can write the integrand as a sum of a polynomial plus a rational function with degree of numerator less than denominator.

Let's perform polynomial division:

Divide \( x^3 \) by \( 3x^2 \): \( \frac{1}{3}x \).

Multiply \( 3x^2 - 3x + 4 \) by \( \frac{1}{3}x \):

\( \frac{1}{3}x \cdot (3x^2 - 3x + 4) = x^3 - x^2 + \frac{4}{3}x \)

Subtract:

\[
\begin{align*}
& x^3 + x + 1 \\
- & (x^3 - x^2 + \frac{4}{3}x) \\
= & (x^3 - x^3) + (0 + x^2) + (x - \frac{4}{3}x) + 1 \\
= & x^2 + (x - \frac{4}{3}x) + 1 \\
= & x^2 - \frac{1}{3}x + 1
\end{align*}
\]

Now divide \( x^2 \) by \( 3x^2 \): \( \frac{1}{3} \).

Multiply \( 3x^2 - 3x + 4 \) by \( \frac{1}{3} \):

\( \frac{1}{3} \cdot (3x^2 - 3x + 4) = x^2 - x + \frac{4}{3} \)

Subtract:

\[
\begin{align*}
& x^2 - \frac{1}{3}x + 1 \\
- & (x^2 - x + \frac{4}{3}) \\
= & (x^2 - x^2) + \left(-\frac{1}{3}x - (-x)\right) + (1 - \frac{4}{3}) \\
= & \left(-\frac{1}{3}x + x\right) + (-\frac{1}{3}) \\
= & \frac{2}{3}x - \frac{1}{3}
\end{align*}
\]

Therefore,
\[
x^3 + x + 1 = (3x^2 - 3x + 4)\left(\frac{1}{3}x + \frac{1}{3}\right) + \left(\frac{2}{3}x - \frac{1}{3}\right)
\]

So,

\[
\frac{x^3 + x + 1}{3x^2 - 3x + 4} = \frac{1}{3}x + \frac{1}{3} + \frac{\frac{2}{3}x - \frac{1}{3}}{3x^2 - 3x + 4}
\]

Rewrite as:

\[
= \frac{1}{3}x + \frac{1}{3} + \frac{2x - 1}{3(3x^2 - 3x + 4)}
\]

**Step 2: Integrate term by term.**

\[
\int_{0}^{1} \frac{x^3 + x + 1}{3x^2 - 3x + 4} dx = \int_{0}^{1} \left( \frac{1}{3}x + \frac{1}{3} + \frac{2x-1}{3(3x^2 - 3x + 4)} \right) dx
\]

\[
= \frac{1}{3} \int_0^1 x \, dx + \frac{1}{3} \int_0^1 dx + \frac{1}{3} \int_0^1 \frac{2x-1}{3x^2 - 3x + 4} dx
\]

Calculate the first two integrals:

\[
\frac{1}{3} \int_0^1 x dx = \frac{1}{3} \left[ \frac{x^2}{2} \right]^1_0 = \frac{1}{3} \cdot \frac{1}{2} = \frac{1}{6}
\]
\[
\frac{1}{3} \int_0^1 dx = \frac{1}{3} [ x ]^1_0 = \frac{1}{3}
\]

So, their sum is:

\[
\frac{1}{6} + \frac{1}{3} = \frac{1}{2}
\]

Now the remaining integral:

\[
\frac{1}{3} \int_0^1 \frac{2x - 1}{3x^2 - 3x + 4} dx
\]

Letâ€™s write numerator \(2x-1\) in terms of the derivative of denominator:

The denominator is \( 3x^2 - 3x + 4 \), its derivative is \( 6x - 3 \).

\( 2x - 1 \) does not exactly match the derivative, but let's express \(2x-1\) as \(a (6x-3)\) plus a constant.

Set
\[
2x - 1 = a(6x - 3) + b
\]
Then,
\[
2x - 1 = 6a x - 3a + b
\]
So,
\[
6a = 2 \implies a = \frac{1}{3}
\]
\[
-3a + b = -1 \implies -1 + b = -1 \implies b = 0
\]
So,
\[
2x-1 = \frac{1}{3}(6x-3)
\]

Therefore,

\[
\frac{2x-1}{3x^2 - 3x + 4} = \frac{1}{3} \cdot \frac{6x-3}{3x^2 - 3x + 4}
\]

Therefore, our integral is:

\[
\frac{1}{3} \int_0^1 \frac{2x-1}{3x^2 - 3x + 4} dx = \frac{1}{3} \cdot \frac{1}{3} \int_0^1 \frac{6x-3}{3x^2 - 3x + 4} dx = \frac{1}{9} \int_0^1 \frac{6x-3}{3x^2 - 3x + 4} dx
\]

Now, observe that \(6x - 3 = d/dx(3x^2 - 3x + 4)\), so

\[
\int \frac{d}{dx}(3x^2 - 3x + 4)}{3x^2 - 3x + 4} dx = \ln|3x^2 - 3x + 4|
\]

So,

\[
\int_0^1 \frac{6x-3}{3x^2 - 3x + 4} dx = \left[ \ln(3x^2 - 3x + 4) \right]_0^1
\]

But \(3x^2 - 3x + 4 > 0\) for all real \(x\), so we can drop the modulus.

Now, let's collect everything:

\[
I = \frac{1}{2} + \frac{1}{9} \left[ \ln(3x^2 - 3x + 4) \right]_0^1
\]

Compute the values at \(x=1\) and \(x=0\):

At \(x=1\):

\[
3(1^2) - 3(1) + 4 = 3 - 3 + 4 = 4
\]

At \(x=0\):

\[
3(0^2) - 3(0) + 4 = 0 - 0 + 4 = 4
\]

Thus,

\[
\left[ \ln(3x^2 - 3x + 4) \right]_0^1 = \ln 4 - \ln 4 = 0
\]

Therefore, the value of the definite integral is simply

\[
\boxed{\frac{1}{2}}
\]

**Numerical approximation:**
\[
\frac{1}{2} = 0.5
\]

**JSON:**
```json
{"answer": "\\frac{1}{2}", "numerical_answer": "0.5"}
```