Let's solve the definite integral:

\[
\int_{1/8}^{1/4} \frac{\ln(2x)\ln(4x)\ln(8x)}{x} \, dx
\]

### Step 1: Simplify the integrand

Express \(\ln(2x)\), \(\ln(4x)\), and \(\ln(8x)\) in terms of \(\ln x\):

- \(\ln(2x) = \ln 2 + \ln x\)
- \(\ln(4x) = \ln 4 + \ln x = 2\ln 2 + \ln x\)
- \(\ln(8x) = \ln 8 + \ln x = 3\ln 2 + \ln x\)

Thus,
\[
I = \int_{1/8}^{1/4} \frac{[\ln 2 + \ln x][2\ln 2 + \ln x][3\ln 2 + \ln x]}{x} dx
\]

Let’s expand this product:

Let \(a = \ln 2\), \(L = \ln x\).
\[
(a + L)(2a + L)(3a + L)
\]

First, expand \((a + L)(2a + L)\):

\[
(a + L)(2a + L) = a(2a + L) + L(2a + L) = 2a^2 + aL + 2aL + L^2 = 2a^2 + 3aL + L^2
\]

Now multiply by \((3a + L)\):

\[
[2a^2 + 3aL + L^2](3a + L)
\]
\[
= 2a^2(3a + L) + 3aL(3a + L) + L^2(3a + L)
\]
\[
= 6a^3 + 2a^2L + 9a^2L + 3aL^2 + 3aL^2 + L^3
\]

Wait, let's expand carefully:

- \(2a^2 \cdot 3a = 6a^3\)
- \(2a^2 \cdot L = 2a^2 L\)
- \(3aL \cdot 3a = 9a^2 L\)
- \(3aL \cdot L = 3aL^2\)
- \(L^2 \cdot 3a = 3aL^2\)
- \(L^2 \cdot L = L^3\)

Sum:

- \(a^3\): \(6a^3\)
- \(a^2 L\): \(2a^2L + 9a^2L = 11a^2L\)
- \(a L^2\): \(3aL^2 + 3aL^2 = 6aL^2\)
- \(L^3\): \(L^3\)

So:

\[
= 6a^3 + 11a^2 L + 6a L^2 + L^3
\]

Recall \(a = \ln 2\), \(L = \ln x\):

\[
\ln(2x)\ln(4x)\ln(8x) = 6(\ln 2)^3 + 11(\ln 2)^2\ln x + 6(\ln 2)(\ln x)^2 + (\ln x)^3
\]

Therefore,

\[
I = \int_{1/8}^{1/4} \frac{6(\ln 2)^3 + 11(\ln 2)^2\ln x + 6(\ln 2)(\ln x)^2 + (\ln x)^3}{x} dx
\]

Split into four integrals:
\[
I = 6 (\ln 2)^3 \int_{1/8}^{1/4} \frac{dx}{x}
+ 11 (\ln 2)^2 \int_{1/8}^{1/4} \frac{\ln x}{x} dx
+ 6 (\ln 2) \int_{1/8}^{1/4} \frac{(\ln x)^2}{x} dx
+ \int_{1/8}^{1/4} \frac{(\ln x)^3}{x} dx
\]

Recall the general formula:
\[
\int \frac{(\ln x)^n}{x} dx = \frac{(\ln x)^{n+1}}{n+1} + C
\]

So:

\[
\int_a^b \frac{(\ln x)^n}{x} dx = \left[ \frac{(\ln x)^{n+1}}{n+1} \right]_a^b
\]

Now apply this for each term:

- \(\int_{1/8}^{1/4} \frac{dx}{x} = [\ln x]_{1/8}^{1/4} = \ln(1/4) - \ln(1/8)\)
- \(\int_{1/8}^{1/4} \frac{\ln x}{x} dx = \left[ \frac{(\ln x)^2}{2} \right]_{1/8}^{1/4}\)
- \(\int_{1/8}^{1/4} \frac{(\ln x)^2}{x} dx = \left[ \frac{(\ln x)^3}{3} \right]_{1/8}^{1/4}\)
- \(\int_{1/8}^{1/4} \frac{(\ln x)^3}{x} dx = \left[ \frac{(\ln x)^4}{4} \right]_{1/8}^{1/4}\)

So:

\[
I = 6 (\ln 2)^3 \left[\ln x\right]_{1/8}^{1/4} + 11 (\ln 2)^2 \left[ \frac{(\ln x)^2}{2} \right]_{1/8}^{1/4} + 6 (\ln 2) \left[ \frac{(\ln x)^3}{3} \right]_{1/8}^{1/4} + \left[ \frac{(\ln x)^4}{4} \right]_{1/8}^{1/4}
\]

Write it more explicitly:

\[
I = 6 (\ln 2)^3 \left(\ln(1/4) - \ln(1/8)\right)
+ 11 (\ln 2)^2 \frac{1}{2} \left[(\ln(1/4))^2 - (\ln(1/8))^2\right]
+ 6 (\ln 2) \frac{1}{3} \left[(\ln(1/4))^3 - (\ln(1/8))^3\right]
+ \frac{1}{4}\left[(\ln(1/4))^4 - (\ln(1/8))^4\right]
\]

Let’s compute \(\ln(1/4)\) and \(\ln(1/8)\):

- \(\ln(1/4) = \ln 1 - \ln 4 = 0 - \ln 4 = -\ln 4\)
- \(\ln(1/8) = \ln 1 - \ln 8 = 0 - \ln 8 = -\ln 8\)

But \(\ln 4 = 2 \ln 2\), \(\ln 8 = 3 \ln 2\), then

- \(\ln(1/4) = -2 \ln 2\)
- \(\ln(1/8) = -3 \ln 2\)

Now compute all necessary powers:

- \((-\alpha)^n = (-1)^n \alpha^n\)
- \((\ln(1/4))^n = (-2 \ln 2)^n\)
- \((\ln(1/8))^n = (-3 \ln 2)^n\)

Now plug into the expression:

\[
I = 6(\ln 2)^3 \left[(-2 \ln 2) - (-3 \ln 2)\right] +  \frac{11}{2}(\ln 2)^2\left[(-2 \ln 2)^2 - (-3 \ln 2)^2\right] \\
+ 2(\ln 2) \left[(-2 \ln 2)^3 - (-3 \ln 2)^3\right] + \frac{1}{4}\left[(-2 \ln 2)^4 - (-3 \ln 2)^4\right]
\]

Now, compute each term separately.

#### 1st term:

\[
6 (\ln 2)^3 \left[ -2 \ln 2 + 3 \ln 2 \right] = 6 (\ln 2)^3 (1 \ln 2) = 6 (\ln 2)^4
\]

#### 2nd term:

First, note

- \((-2 \ln 2)^2 = 4 (\ln 2)^2\)
- \((-3 \ln 2)^2 = 9 (\ln 2)^2\)
- The difference: \(4 (\ln 2)^2 - 9 (\ln 2)^2 = -5 (\ln 2)^2\)

So:

\[
\frac{11}{2}(\ln 2)^2 \cdot [-5 (\ln 2)^2] = -\frac{55}{2} (\ln 2)^4
\]

#### 3rd term:

Compute the cubes:

- \((-2 \ln 2)^3 = -8 (\ln 2)^3\)
- \((-3 \ln 2)^3 = -27 (\ln 2)^3\)
- The difference: \(-8 - (-27) = 19\), so \(19 (\ln 2)^3\)

So:

\[
2 (\ln 2) \cdot 19 (\ln 2)^3 = 38 (\ln 2)^4
\]

#### 4th term:

Fourth powers:

- \((-2 \ln 2)^4 = 16 (\ln 2)^4\)
- \((-3 \ln 2)^4 = 81 (\ln 2)^4\)
- The difference: \(16 - 81 = -65\), so \(-65 (\ln 2)^4\)

So:

\[
\frac{1}{4} \cdot [-65 (\ln 2)^4] = -\frac{65}{4} (\ln 2)^4
\]

#### Put it all together:

Now sum up all terms:

\[
I = 6 (\ln 2)^4 - \frac{55}{2} (\ln 2)^4 + 38 (\ln 2)^4 - \frac{65}{4} (\ln 2)^4
\]

\[
= \left( 6 - \frac{55}{2} + 38 - \frac{65}{4} \right) (\ln 2)^4
\]

Compute the sum:

First, write all terms with denominator 4:

- \(6 = 24/4\)
- \(-\frac{55}{2} = -110/4\)
- \(38 = 152/4\)
- \(-\frac{65}{4}\)

Sum:

\[
24/4 - 110/4 + 152/4 - 65/4 = (24 - 110 + 152 - 65)/4 = (24 + 152) - (110 + 65) = 176 - 175 = 1/4
\]

So,

\[
I = \frac{1}{4} (\ln 2)^4
\]

### Step 2: Final exact answer

\[
\boxed{I = \frac{1}{4} (\ln 2)^4}
\]

### Step 3: Numerical approximation

Calculate \((\ln 2)^4\):

- \(\ln 2 \approx 0.6931471805599453\)
- \((\ln 2)^4 \approx (0.6931471805599453)^4 \approx 0.2310490601866484\)
- So, \(I \approx \frac{1}{4} \times 0.2310490601866484 = 0.0577622650466621\)

Rounded to ten decimal places:

\[
I \approx 0.0577622650
\]

### Step 4: JSON Output

```json
{"answer": "\\frac{1}{4} (\\ln 2)^4", "numerical_answer": "0.0577622650"}
```