We start with the given integral

  I = ∫₀¹ (x − 1)² (x + 1)² (x² + 1)² (x⁴ + 1)² dx.

Step 1. Notice that
  (x − 1)² (x + 1)² = (x² − 1)².
Thus the integrand becomes
  (x² − 1)² (x² + 1)² (x⁴ + 1)².

Step 2. Combine the first two factors:
  (x² − 1)² (x² + 1)² = ((x² − 1)(x² + 1))² = (x⁴ − 1)².
So the integrand simplifies to
  (x⁴ − 1)² (x⁴ + 1)².

Step 3. Multiply these two factors:
  (x⁴ − 1)(x⁴ + 1) = x⁸ − 1,
thus
  (x⁴ − 1)² (x⁴ + 1)² = (x⁸ − 1)².
Since squaring removes the sign,
  (x⁸ − 1)² = (1 − x⁸)².

Step 4. Expand (1 − x⁸)²:
  (1 − x⁸)² = 1 − 2x⁸ + x¹⁶.
Then the integral becomes
  I = ∫₀¹ [1 − 2x⁸ + x¹⁶] dx.

Step 5. Integrate term by term:
  ∫₀¹ 1 dx = 1,
  ∫₀¹ x⁸ dx = 1/9,
  ∫₀¹ x¹⁶ dx = 1/17.
So,
  I = 1 − 2(1/9) + 1/17 = 1 − 2/9 + 1/17.

Step 6. Combine the terms with a common denominator. The common denominator for 9 and 17 is 153:
  1 = 153/153,
  2/9 = 34/153,
  1/17 = 9/153.
Thus,
  I = (153 − 34 + 9)/153 = 128/153.

Step 7. Numerical approximation:
  128/153 ≈ 0.8366013072.

The final answers are provided below in the required JSON format.

{"answer": "\\frac{128}{153}", "numerical_answer": "0.8366013072"}