<think>
Okay, let's tackle this integral step by step. The integral given is from 0 to 2.0 of x^(1/2) times (2.0 - x)^(-1/2) multiplied by the natural logarithm of [1.0 times the square root of x(2.0 - x) plus the square root of 1 + (1.0)^2 times x(2.0 - x)] dx. Hmm, that's a mouthful. Let me parse this carefully.

First, let's rewrite the integral in a more manageable form. The integrand is x^(1/2)(2 - x)^(-1/2) ln( sqrt(x(2 - x)) + sqrt(1 + x(2 - x)) ). Wait, the 1.0 coefficients can be considered as 1, so maybe simplifying that part. Let me check: the argument inside the log is 1.0*sqrt(x(2 - x)) + sqrt(1 + 1.0^2 x(2 - x)). Since 1.0 squared is 1, that simplifies to sqrt(x(2 - x)) + sqrt(1 + x(2 - x)). So the integrand becomes x^(1/2) (2 - x)^(-1/2) ln( sqrt(x(2 - x)) + sqrt(1 + x(2 - x)) ) dx from 0 to 2.

Hmm, maybe a substitution would help here. Let's consider the substitution t = x/(2 - x). Wait, but the term (2 - x) is in the denominator. Alternatively, maybe a trigonometric substitution. Let me think. The limits are from 0 to 2, and the integrand has x^(1/2) and (2 - x)^(-1/2). Let me try substituting x = 2 sin^2 θ. Then dx = 4 sin θ cos θ dθ. Let's see:

If x = 2 sin^2 θ, then when x = 0, θ = 0, and when x = 2, θ = π/2. Let's compute the terms:

sqrt(x) = sqrt(2 sin^2 θ) = sqrt(2) sin θ.

(2 - x)^(-1/2) = (2 - 2 sin^2 θ)^(-1/2) = (2 cos^2 θ)^(-1/2) = 1/(sqrt(2) cos θ).

The argument inside the log becomes sqrt(x(2 - x)) + sqrt(1 + x(2 - x)).

Compute x(2 - x) = 2 sin^2 θ * 2 cos^2 θ = 4 sin^2 θ cos^2 θ. So sqrt(x(2 - x)) = 2 sin θ cos θ.

Then sqrt(1 + x(2 - x)) = sqrt(1 + 4 sin^2 θ cos^2 θ). Hmm, maybe simplify that expression. Let's note that 4 sin^2 θ cos^2 θ = sin^2(2θ). So 1 + sin^2(2θ). But sqrt(1 + sin^2(2θ)) doesn't immediately simplify. Wait, but maybe there's a hyperbolic identity here. Alternatively, perhaps the argument inside the log can be expressed as sinh or cosh. Let me think: sqrt(a) + sqrt(1 + a). Let me set a = x(2 - x). Then the argument is sqrt(a) + sqrt(1 + a). Let me compute that expression. Let's denote sqrt(a) = t. Then the expression becomes t + sqrt(1 + t^2). Wait, that's the definition of sinh^{-1}(t) + t? Wait, actually, sinh(u) = t, then sqrt(1 + t^2) = cosh(u), so t + sqrt(1 + t^2) = sinh(u) + cosh(u) = e^u. So ln(t + sqrt(1 + t^2)) = u. But u = sinh^{-1}(t). Therefore, ln(sqrt(a) + sqrt(1 + a)) = sinh^{-1}(sqrt(a)). Alternatively, since sinh^{-1}(z) = ln(z + sqrt(z^2 + 1)), which is exactly the expression here. Therefore, the logarithm term simplifies to sinh^{-1}(sqrt(a)) where a = x(2 - x). So the integrand becomes x^(1/2) (2 - x)^(-1/2) sinh^{-1}(sqrt(x(2 - x))).

But maybe this substitution helps. Let's proceed with the substitution x = 2 sin^2 θ. Then, as before, dx = 4 sin θ cos θ dθ. Let's substitute all terms into the integral:

Integral from θ=0 to θ=π/2 of [sqrt(2) sin θ] * [1/(sqrt(2) cos θ)] * sinh^{-1}(2 sin θ cos θ) * 4 sin θ cos θ dθ.

Simplify term by term:

sqrt(2) sin θ * 1/(sqrt(2) cos θ) = (sqrt(2)/sqrt(2)) (sin θ / cos θ) = tan θ.

Then multiplied by 4 sin θ cos θ: tan θ * 4 sin θ cos θ = 4 sin^2 θ.

So the integral becomes 4 ∫ sin^2 θ sinh^{-1}(2 sin θ cos θ) dθ from 0 to π/2.

Wait, 2 sin θ cos θ is sin(2θ). So sinh^{-1}(sin(2θ)). Therefore, the integral becomes 4 ∫ sin^2 θ sinh^{-1}(sin(2θ)) dθ from 0 to π/2.

Hmm, that seems a bit complicated, but maybe there's a way to simplify sinh^{-1}(sin(2θ)). Let's recall that sinh^{-1}(z) = ln(z + sqrt(z^2 + 1)). So sinh^{-1}(sin(2θ)) = ln(sin(2θ) + sqrt(sin^2(2θ) + 1)). Let's compute sqrt(sin^2(2θ) + 1). That's sqrt(1 + sin^2(2θ)). Hmm, not sure if that simplifies. Alternatively, maybe another substitution. Let me think.

Alternatively, perhaps integrating by parts. Let's consider the integral 4 ∫ sin^2 θ sinh^{-1}(sin(2θ)) dθ. Let me set u = sinh^{-1}(sin(2θ)), dv = 4 sin^2 θ dθ. Then du = derivative of sinh^{-1}(sin(2θ)) dθ. Let's compute du:

d/dθ sinh^{-1}(z) = (1 / sqrt(z^2 + 1)) dz/dθ. Here z = sin(2θ), so dz/dθ = 2 cos(2θ). Therefore, du = [2 cos(2θ) / sqrt(sin^2(2θ) + 1)] dθ.

And v would be the integral of 4 sin^2 θ dθ. Let's compute that:

Integral of 4 sin^2 θ dθ = 4 * (θ/2 - sin(2θ)/4) + C = 2θ - sin(2θ) + C.

So integrating by parts, we get:

u*v | from 0 to π/2 - ∫ v du.

So:

4 [ sinh^{-1}(sin(2θ)) * (2θ - sin(2θ)) evaluated from 0 to π/2 - ∫ (2θ - sin(2θ)) * (2 cos(2θ) / sqrt(sin^2(2θ) + 1)) dθ ]

Let's evaluate the boundary term first. At θ = π/2, sin(2θ) = sin(π) = 0, so sinh^{-1}(0) = 0. At θ = 0, sin(0) = 0, so sinh^{-1}(0) = 0. Therefore, the boundary term is 0 - 0 = 0. So the integral reduces to:

-4 ∫ (2θ - sin(2θ)) * (2 cos(2θ) / sqrt(sin^2(2θ) + 1)) dθ from 0 to π/2.

Simplify the constants: -4 * 2 = -8, so:

-8 ∫ (2θ - sin(2θ)) * (cos(2θ) / sqrt(sin^2(2θ) + 1)) dθ.

Hmm, this seems more complicated. Maybe another substitution. Let me set t = 2θ. Then when θ = 0, t = 0; θ = π/2, t = π. Then dθ = dt/2. The integral becomes:

-8 ∫ (t - sin t) * (cos t / sqrt(sin^2 t + 1)) * (dt/2) from t=0 to t=π.

Simplify: -8 * (1/2) ∫ (t - sin t) * (cos t / sqrt(sin^2 t + 1)) dt from 0 to π.

Which is -4 ∫ (t - sin t) * (cos t / sqrt(sin^2 t + 1)) dt from 0 to π.

Hmm, this still looks challenging. Let's split the integral into two parts:

-4 [ ∫ t cos t / sqrt(sin^2 t + 1) dt - ∫ sin t cos t / sqrt(sin^2 t + 1) dt ] from 0 to π.

Let me handle each integral separately. Let's first compute the second integral: ∫ sin t cos t / sqrt(sin^2 t + 1) dt.

Let u = sin t, then du = cos t dt. Then the integral becomes ∫ u / sqrt(u^2 + 1) du. That's straightforward. The integral of u / sqrt(u^2 + 1) du is sqrt(u^2 + 1) + C. So evaluated from 0 to π, which is [sqrt(sin^2 π + 1) - sqrt(sin^2 0 + 1)] = sqrt(0 + 1) - sqrt(0 + 1) = 1 - 1 = 0. So the second integral is 0.

So now we have -4 [ ∫ t cos t / sqrt(sin^2 t + 1) dt - 0 ] from 0 to π. So the integral reduces to -4 ∫ t cos t / sqrt(sin^2 t + 1) dt from 0 to π.

Hmm, this integral is still non-trivial. Let's consider substitution. Let me set u = sin t. Then du = cos t dt. But we have a t term, which complicates things. Alternatively, perhaps another substitution. Let me note that sqrt(sin^2 t + 1) = sqrt(1 + sin^2 t). Hmm, not sure. Alternatively, perhaps integrating by parts again. Let me set for the integral ∫ t cos t / sqrt(1 + sin^2 t) dt.

Let me set u = t, dv = cos t / sqrt(1 + sin^2 t) dt.

Then du = dt, and v = ∫ cos t / sqrt(1 + sin^2 t) dt.

Compute v: Let w = sin t, dw = cos t dt. Then v = ∫ dw / sqrt(1 + w^2) = sinh^{-1}(w) + C = sinh^{-1}(sin t) + C.

Therefore, integrating by parts:

u*v - ∫ v du = t sinh^{-1}(sin t) - ∫ sinh^{-1}(sin t) dt.

So the integral becomes:

-4 [ t sinh^{-1}(sin t) | from 0 to π - ∫ sinh^{-1}(sin t) dt from 0 to π ].

Evaluate the boundary term: At t = π, sinh^{-1}(sin π) = sinh^{-1}(0) = 0. At t = 0, sinh^{-1}(0) = 0. So the boundary term is 0 - 0 = 0. Therefore, the integral reduces to:

-4 [ - ∫ sinh^{-1}(sin t) dt from 0 to π ] = 4 ∫ sinh^{-1}(sin t) dt from 0 to π.

So now we have to compute ∫ sinh^{-1}(sin t) dt from 0 to π. Hmm, interesting. Let's analyze sinh^{-1}(sin t). Let's recall that sinh^{-1}(x) = ln(x + sqrt(x^2 + 1)). So sinh^{-1}(sin t) = ln(sin t + sqrt(sin^2 t + 1)).

But sinh^{-1}(sin t) is not a standard function, but perhaps we can relate it to t. Let's consider the expression sinh^{-1}(sin t). Let me see if there's a relationship between sinh^{-1}(sin t) and t. Let's compute sinh(s) = sin t, then s = sinh^{-1}(sin t). But sinh(s) = sin t. Then s = sinh^{-1}(sin t). Hmm, not sure. Alternatively, perhaps consider specific intervals. For t in [0, π/2], sin t is increasing from 0 to 1. For t in [π/2, π], sin t is decreasing from 1 to 0. Let's see if sinh^{-1}(sin t) can be expressed in terms of t.

Wait, let's compute sinh^{-1}(sin t) for t in [0, π/2]. Let’s set t = sinh^{-1}(sin t). Wait, that's not helpful. Alternatively, maybe use a substitution. Let me consider that sinh^{-1}(x) = ln(x + sqrt(x^2 + 1)). So sinh^{-1}(sin t) = ln(sin t + sqrt(sin^2 t + 1)). Let's compute sqrt(sin^2 t + 1). That's sqrt(1 + sin^2 t). Hmm, not sure. Alternatively, maybe relate to hyperbolic functions. Let me think.

Alternatively, perhaps consider that sinh^{-1}(sin t) can be expressed as a function of t. Let me check for specific values. For t = 0: sinh^{-1}(0) = 0. For t = π/2: sinh^{-1}(1) = ln(1 + sqrt(2)). For t = π: sinh^{-1}(0) = 0. Hmm, so the function sinh^{-1}(sin t) is symmetric around t = π/2. Let's see if integrating from 0 to π can be simplified by symmetry.

Let’s split the integral into two parts: from 0 to π/2 and π/2 to π. Let’s make a substitution in the second interval. Let u = π - t in the interval π/2 to π. Then when t = π/2, u = π/2; t = π, u = 0. Then du = -dt. The integral becomes:

∫_{π/2}^{π} sinh^{-1}(sin t) dt = ∫_{0}^{π/2} sinh^{-1}(sin(π - u)) (-du) = ∫_{0}^{π/2} sinh^{-1}(sin u) du.

Because sin(π - u) = sin u. Therefore, the integral from 0 to π is 2 times the integral from 0 to π/2 of sinh^{-1}(sin t) dt.

So, 4 * 2 ∫_{0}^{π/2} sinh^{-1}(sin t) dt = 8 ∫_{0}^{π/2} sinh^{-1}(sin t) dt.

Wait, no. Wait, the original integral after substitution became 4 ∫_{0}^{π} sinh^{-1}(sin t) dt. But splitting into two parts, we have 4 * [ ∫_{0}^{π/2} sinh^{-1}(sin t) dt + ∫_{π/2}^{π} sinh^{-1}(sin t) dt ] = 4 * [ ∫_{0}^{π/2} sinh^{-1}(sin t) dt + ∫_{0}^{π/2} sinh^{-1}(sin u) du ] = 8 ∫_{0}^{π/2} sinh^{-1}(sin t) dt.

So the integral is 8 ∫_{0}^{π/2} sinh^{-1}(sin t) dt. Hmm, but how to compute this integral?

Let me consider integrating sinh^{-1}(sin t) from 0 to π/2. Let's make a substitution. Let’s set u = t. Wait, not helpful. Alternatively, integrate by parts. Let’s set u = sinh^{-1}(sin t), dv = dt. Then du = [cos t / sqrt(sin^2 t + 1)] dt, and v = t.

Integrating by parts: uv | from 0 to π/2 - ∫ v du = t sinh^{-1}(sin t) | from 0 to π/2 - ∫ t [cos t / sqrt(sin^2 t + 1)] dt.

Evaluate the boundary term: At π/2, sinh^{-1}(1) = ln(1 + sqrt(2)), multiplied by π/2. At 0, sinh^{-1}(0) = 0. So boundary term is (π/2) ln(1 + sqrt(2)) - 0 = (π/2) ln(1 + sqrt(2)).

So the integral becomes:

(π/2) ln(1 + sqrt(2)) - ∫_{0}^{π/2} [t cos t / sqrt(sin^2 t + 1)] dt.

But this integral is similar to the one we had earlier. Wait, but this is the same integral we encountered before. Hmm, this seems like we're going in circles. Let me check.

Wait, the original integral after substitution became 8 times the integral of sinh^{-1}(sin t) from 0 to π/2. But integrating by parts, we have:

8 [ (π/2) ln(1 + sqrt(2)) - ∫_{0}^{π/2} t cos t / sqrt(sin^2 t + 1) dt ].

But this integral ∫ t cos t / sqrt(sin^2 t + 1) dt from 0 to π/2 is part of the expression we had earlier. Wait, but this seems recursive. Maybe there's a different approach.

Alternatively, perhaps consider a substitution in the integral ∫ sinh^{-1}(sin t) dt. Let me think about the expression sinh^{-1}(sin t). Let's recall that sinh^{-1}(x) = ln(x + sqrt(x^2 + 1)). So sinh^{-1}(sin t) = ln(sin t + sqrt(sin^2 t + 1)). Let's compute this expression:

sqrt(sin^2 t + 1) = sqrt(1 + sin^2 t). Hmm, not sure. Alternatively, maybe relate to hyperbolic functions. Let me set sinh y = sin t. Then y = sinh^{-1}(sin t). Then cosh y = sqrt(1 + sinh^2 y) = sqrt(1 + sin^2 t). Then sinh y = sin t. Then, perhaps express y in terms of t. But I don't see a direct relationship.

Alternatively, consider expanding sinh^{-1}(sin t) in a series. But that might not be helpful for an exact solution.

Wait, perhaps there's a trick here. Let me recall that the original integral was transformed through substitution into 8 ∫_{0}^{π/2} sinh^{-1}(sin t) dt. If we can compute this integral, we can find the answer.

Alternatively, maybe consider differentiating under the integral sign. Let me define I(a) = ∫_{0}^{π/2} sinh^{-1}(a sin t) dt. Then compute I(1). Then find I'(a) = ∫_{0}^{π/2} [ sin t / sqrt(a^2 sin^2 t + 1) ] dt. Hmm, but integrating this might be complicated. Let's try:

I'(a) = ∫_{0}^{π/2} [ sin t / sqrt(a^2 sin^2 t + 1) ] dt.

Let me substitute u = cos t, then du = -sin t dt. When t=0, u=1; t=π/2, u=0. So:

I'(a) = ∫_{u=1}^{0} [ -du / sqrt(a^2 (1 - u^2) + 1) ] = ∫_{0}^{1} [ 1 / sqrt(a^2 (1 - u^2) + 1) ] du.

Simplify the denominator: a^2 (1 - u^2) + 1 = a^2 + 1 - a^2 u^2 = (a^2 + 1) - a^2 u^2. So:

I'(a) = ∫_{0}^{1} 1 / sqrt( (a^2 + 1) - a^2 u^2 ) du.

This is a standard integral. The integral of 1 / sqrt(c - d u^2) du is (1/√d) sin^{-1}(u sqrt(d/c)) ) + C, for c, d > 0. Let's check:

Let’s set c = a^2 + 1, d = a^2. Then:

I'(a) = ∫_{0}^{1} 1 / sqrt(c - d u^2) du = [ (1/√d) sin^{-1}(u sqrt(d/c)) ) ] from 0 to 1.

At u=1: (1/√d) sin^{-1}( sqrt(d/c) ) = (1/a) sin^{-1}( a / sqrt(a^2 + 1) ).

At u=0: 0. So:

I'(a) = (1/a) sin^{-1}( a / sqrt(a^2 + 1) ).

But sin^{-1}(a / sqrt(a^2 + 1)) is equal to tan^{-1}(a). Because if θ = sin^{-1}(a / sqrt(a^2 + 1)), then sin θ = a / sqrt(a^2 + 1), so tan θ = a / 1, so θ = tan^{-1}(a). Therefore:

I'(a) = (1/a) tan^{-1}(a).

Therefore, I(a) = ∫ (1/a) tan^{-1}(a) da + C. Let's compute this integral.

Let’s integrate (1/a) tan^{-1}(a) da. Let’s use integration by parts. Let u = tan^{-1}(a), dv = (1/a) da. Then du = 1/(1 + a^2) da, v = ln |a|.

So ∫ (1/a) tan^{-1}(a) da = tan^{-1}(a) ln a - ∫ ln a / (1 + a^2) da.

Hmm, the integral ∫ ln a / (1 + a^2) da. Let me consider substitution. Let’s set t = a^2. Not sure. Alternatively, note that ∫ ln a / (1 + a^2) da from 0 to infinity is known, but here we have indefinite integral. Alternatively, perhaps expand in series. But this seems complicated. Alternatively, recall that ∫ ln a / (1 + a^2) da = -Im(Li_2(ia)) + C, but this is getting into polylogarithms, which might not be helpful for an exact answer.

Alternatively, perhaps consider that the integral I(a) is defined as ∫_{0}^{π/2} sinh^{-1}(a sin t) dt. We need to find I(1). But since we have I'(a) = (1/a) tan^{-1}(a), then integrating from a=0 to a=1:

I(1) - I(0) = ∫_{0}^{1} (1/a) tan^{-1}(a) da.

But I(0) = ∫_{0}^{π/2} sinh^{-1}(0) dt = 0. So I(1) = ∫_{0}^{1} (1/a) tan^{-1}(a) da.

So we need to compute ∫_{0}^{1} (tan^{-1}(a)/a) da. Let's make a substitution. Let’s set u = tan^{-1}(a). Then a = tan u, da = sec^2 u du. When a=0, u=0; a=1, u=π/4. The integral becomes:

∫_{0}^{π/4} (u / tan u) * sec^2 u du = ∫_{0}^{π/4} u * (sec^2 u / tan u) du = ∫_{0}^{π/4} u * (1/(sin u cos u)) du.

Since sec^2 u = 1 + tan^2 u, but here sec^2 u / tan u = (1 + tan^2 u)/tan u = cot u + tan u. Wait, but maybe simplify:

sec^2 u / tan u = (1/cos^2 u) / (sin u / cos u) ) = 1/(sin u cos u). So the integral becomes ∫_{0}^{π/4} u / (sin u cos u) du.

But 1/(sin u cos u) = 2 / sin(2u). So:

∫_{0}^{π/4} 2u / sin(2u) du.

Let’s substitute v = 2u, dv = 2 du, so du = dv/2. When u=0, v=0; u=π/4, v=π/2. The integral becomes:

∫_{0}^{π/2} (v/2) / sin v * (dv/2) ) = (1/4) ∫_{0}^{π/2} v / sin v dv.

Hmm, the integral ∫ v / sin v dv is known to be related to the Clausen function, but I'm not sure if that's helpful here. Alternatively, perhaps expand 1/sin v as a series. Recall that 1/sin v = csc v = 2/(e^{iv} - e^{-iv}) ), but maybe using a series expansion.

Alternatively, recall that 1/sin v can be expressed as a sum from n=0 to ∞ of 2/(v - nπ)) for residues, but that might not be helpful. Alternatively, use the expansion of csc v as a series:

For 0 < v < π, csc v = 1/v + 2v/π^2 Σ_{k=1}^∞ (-1)^{k+1} (π^2 - v^2)/(k^2 π^2 - v^2). Hmm, not sure.

Alternatively, use integration by parts again. Let’s set w = v, dz = 1/sin v dv. Then dw = dv, and z = ln |tan(v/2)|. So:

∫ v / sin v dv = v ln(tan(v/2)) - ∫ ln(tan(v/2)) dv.

But this seems more complicated. Alternatively, perhaps consider expanding in a power series. Let's recall that for 0 < v < π, 1/sin v = 2 Σ_{n=0}^∞ sin((2n+1)v)/(2n+1). Wait, that's the Fourier series expansion of csc v. So:

1/sin v = 2 Σ_{n=0}^∞ sin((2n+1)v) for 0 < v < π.

Therefore, ∫_{0}^{π/2} v / sin v dv = 2 ∫_{0}^{π/2} v Σ_{n=0}^∞ sin((2n+1)v) dv.

Interchange sum and integral:

2 Σ_{n=0}^∞ ∫_{0}^{π/2} v sin((2n+1)v) dv.

Integrate by parts: Let’s set u = v, dv = sin((2n+1)v) dv. Then du = dv, v = -cos((2n+1)v)/(2n+1).

Wait, integral of sin(kv) dv = -cos(kv)/k. So:

∫ v sin(kv) dv = -v cos(kv)/k + ∫ cos(kv)/k dv = -v cos(kv)/k + sin(kv)/k^2 + C.

So for k = 2n+1:

∫_{0}^{π/2} v sin((2n+1)v) dv = [ -v cos((2n+1)v)/(2n+1) + sin((2n+1)v)/(2n+1)^2 ] from 0 to π/2.

At v=π/2:

First term: -π/2 * cos((2n+1)π/2) / (2n+1). Cos((2n+1)π/2) = 0 for all integers n, because (2n+1)π/2 is an odd multiple of π/2, where cosine is zero.

Second term: sin((2n+1)π/2)/(2n+1)^2. Sin((2n+1)π/2) = sin(nπ + π/2) = (-1)^n.

At v=0:

First term: 0.

Second term: sin(0)/(2n+1)^2 = 0.

Therefore, the integral evaluates to [0 + (-1)^n/(2n+1)^2] - [0 + 0] = (-1)^n/(2n+1)^2.

Therefore, the sum becomes:

2 Σ_{n=0}^∞ [ (-1)^n / (2n+1)^2 ].

So the integral ∫_{0}^{π/2} v / sin v dv = 2 Σ_{n=0}^∞ [ (-1)^n / (2n+1)^2 ].

This series is known. It's related to the Dirichlet beta function. Specifically, β(2) = Σ_{n=0}^∞ (-1)^n / (2n+1)^2. This is known as Catalan's constant, G. However, Catalan's constant is approximately 0.9159655942... and it's not expressible in terms of elementary functions. Therefore, the integral ∫_{0}^{π/2} v / sin v dv = 2G.

But going back, our original integral I(1) = ∫_{0}^{1} (tan^{-1}(a)/a) da = (1/4) ∫_{0}^{π/2} v / sin v dv = (1/4)(2G) = G/2.

Wait, no. Let's retrace:

We had I(1) = ∫_{0}^{1} (tan^{-1}(a)/a) da = (1/4) ∫_{0}^{π/2} v / sin v dv = (1/4)(2G) = G/2.

But Catalan's constant G is Σ_{n=0}^∞ (-1)^n / (2n+1)^2 ≈ 0.9159655942. Therefore, I(1) = G/2 ≈ 0.4579827971.

But wait, this seems to suggest that the original integral 8 * I(1) = 8 * (G/2) = 4G. But the original integral after substitution was 8 ∫_{0}^{π/2} sinh^{-1}(sin t) dt = 8 * I(1) = 4G. Therefore, the value of the original definite integral is 4G, where G is Catalan's constant.

But wait, let's confirm:

Original integral was:

Integral from 0 to 2 of x^{1/2}(2 - x)^{-1/2} ln(...) dx = 4G.

But wait, let's check the steps again. The original integral after substitution became 8 ∫_{0}^{π/2} sinh^{-1}(sin t) dt. Then, through various substitutions and integration by parts, we found that this equals 4G. Therefore, the exact value of the integral is 4 times Catalan's constant.

But wait, let's verify the steps:

Original integral transformed via substitution x=2 sin^2 θ into 4 ∫ sinh^{-1}(sin 2θ) sin^2 θ dθ from 0 to π/2. Then through multiple substitutions and integration by parts, we arrived at 4G. But according to the steps above, after multiple substitutions and recognizing the Catalan's constant, the integral evaluates to 4G.

Therefore, the exact answer is 4G, where G is Catalan's constant. However, since the problem asks for the exact answer in LaTeX, we need to express it in terms of Catalan's constant. But if the problem expects a numerical value, we can use the approximate value of G ≈ 0.915965594177219... So 4G ≈ 3.663862376708876.

But let's check the numerical approximation. Let's compute the integral numerically to verify.

Alternatively, perhaps there's a mistake in the steps. Let me verify the key steps.

We started with the integral, substituted x = 2 sin^2 θ, transformed the integral into 4 ∫ sinh^{-1}(sin 2θ) sin^2 θ dθ from 0 to π/2. Then through integration by parts and substitutions, we arrived at 4G. But let's verify with a numerical check.

Let me compute the original integral numerically. Let's approximate the integral from 0 to 2 of sqrt(x) / sqrt(2 - x) * ln(sqrt(x(2 - x)) + sqrt(1 + x(2 - x))) dx.

Let's use numerical integration. For example, using a calculator or software. But since I can't compute it here, I'll rely on the analytical steps. Given that the integral reduces to 4G, and G is approximately 0.9159655942, then 4G ≈ 3.6638623768.

But let me check if there's a known integral that results in Catalan's constant. Yes, some integrals involving inverse hyperbolic functions and trigonometric functions do result in Catalan's constant. For example, ∫_{0}^{π/2} t / sin t dt = 2G. But in our case, after substitutions, we arrived at 4G. Therefore, the exact answer is 4G, which is 4 times Catalan's constant.

Therefore, the exact answer is 4G, and the numerical approximation is approximately 3.6638623767.

But let me check if there's a mistake in the sign. Because during integration by parts, there were negative signs. Let me retrace:

Original integral after substitution became 4 ∫ sinh^{-1}(sin 2θ) sin^2 θ dθ. Then integrating by parts, we ended up with 4 ∫ sinh^{-1}(sin t) dt from 0 to π, which became 8 ∫ sinh^{-1}(sin t) dt from 0 to π/2. Then through integrating I(a) and finding I(1) = G/2, then 8 * I(1) = 4G. So yes, the exact answer is 4G.

Therefore, the exact answer is 4G, which is 4 times Catalan's constant. The numerical value is approximately 4 * 0.915965594177219 ≈ 3.663862376708876. Rounded to 10 decimal places, that's 3.6638623767.

But let me verify with another approach. Let's consider the original integrand:

x^{1/2} (2 - x)^{-1/2} ln(sqrt(x(2 - x)) + sqrt(1 + x(2 - x))).

Let me make a substitution y = x/2, so x = 2y, dx = 2 dy. Then the integral becomes from y=0 to y=1:

sqrt(2y) * (2 - 2y)^{-1/2} * ln( sqrt(2y * 2(1 - y)) + sqrt(1 + 2y * 2(1 - y)) ) * 2 dy.

Simplify:

sqrt(2y) = sqrt(2) sqrt(y).

(2 - 2y)^{-1/2} = (2(1 - y))^{-1/2} = 1/(sqrt(2) sqrt(1 - y)).

Multiply by 2 dy: sqrt(2) sqrt(y) * 1/(sqrt(2) sqrt(1 - y)) * 2 dy = 2 sqrt(y/(1 - y)) dy.

The argument inside the log becomes sqrt(2y * 2(1 - y)) + sqrt(1 + 2y * 2(1 - y)).

Simplify:

sqrt(4y(1 - y)) = 2 sqrt(y(1 - y)).

Inside the sqrt(1 + 4y(1 - y)): 1 + 4y(1 - y) = 1 + 4y - 4y^2 = -4y^2 +4y +1. Hmm, not sure. Alternatively, note that 4y(1 - y) = 4y -4y^2. So sqrt(1 +4y(1 - y)) = sqrt(1 +4y -4y^2) = sqrt(-4y^2 +4y +1). Not sure if that helps.

But the argument inside the log is 2 sqrt(y(1 - y)) + sqrt(1 +4y(1 - y)).

But this substitution doesn't seem to simplify things further. However, the previous analytical steps leading to 4G seem correct, so I'll proceed with that.

Therefore, the exact answer is 4G, and the numerical approximation is approximately 3.6638623767.
</think>

{"answer": "4G", "numerical_answer": "3.6638623767"}