We will show that

  I = ∫₀² x^(–1) · arctan(√(x(2–x))) dx = π ln(1 + √2).

In what follows we describe one route leading to this answer.

Step 1. Make a Change of Variable

The original integral is
  I = ∫₀² (1/x) arctan(√(x(2–x))) dx.
Make the shift
  u = x – 1  so that x = u + 1.
Then the limits become u = –1 (when x = 0) and u = 1 (when x = 2). Notice that
  x(2–x) = (u + 1)[2 – (u + 1)] = (u + 1)(1 – u) = 1 – u².
Thus the integral becomes
  I = ∫_{u=–1}^{1} [1/(u+1)] arctan(√(1–u²)) du.

Step 2. Symmetrize the Integral

Notice that the integrand (as a function of u) is not even because of the factor 1/(u+1). However one may write it as the average of two expressions. In fact, if one makes the change u → –u in the integrand one obtains
  I = ∫_{–1}^{1} [1/(1–u)] arctan(√(1–u²)) du.
Averaging the two forms we deduce that
  I = (1/2) ∫_{–1}^{1} [1/(1+u) + 1/(1–u)] arctan(√(1–u²)) du.
But
  1/(1+u) + 1/(1–u) = (1–u + 1+u)/(1–u²) = 2/(1–u²).
Thus,
  I = (1/2) ∫_{–1}^{1} [2/(1–u²)] arctan(√(1–u²)) du = ∫_{–1}^{1} [1/(1–u²)] arctan(√(1–u²)) du.
Since the integrand is now even, we may write
  I = 2 ∫₀¹ [1/(1–u²)] arctan(√(1–u²)) du.

Step 3. A Trigonometric Substitution

Make the substitution
  u = cosθ,  with du = –sinθ dθ.
When u goes from 0 to 1 the variable θ goes from π/2 to 0. Also,
  1 – u² = 1 – cos²θ = sin²θ  and  √(1–u²) = sinθ.
Thus,
  I = 2 ∫_{θ=π/2}^{0} [1/sin²θ] arctan(sinθ) · (–sinθ dθ)
     = 2 ∫₀^{π/2} [arctan(sinθ)/sinθ] dθ.
That is,
  I = 2 ∫₀^(π/2) [arctan(sinθ)/sinθ] dθ.

Step 4. Represent arctan(sinθ) as an Integral

A useful representation is
  arctan z = ∫₀¹ [z/(1 + t² z²)] dt  for any z.
Using z = sinθ we have
  arctan(sinθ) = ∫₀¹ [sinθ/(1 + t² sin²θ)] dt.
Substitute this into I:
  I = 2 ∫₀^(π/2) [1/sinθ] {∫₀¹ [sinθ/(1 + t² sin²θ)] dt} dθ
    = 2 ∫₀¹ {∫₀^(π/2) [dθ/(1 + t² sin²θ)]} dt.
We may interchange the integrals (by Fubini’s theorem):
  I = 2 ∫₀¹ J(t) dt,  where J(t) = ∫₀^(π/2) [dθ/(1 + t² sin²θ)].

Step 5. The θ–Integral

The inner integral is classical. In fact, one standard result is
  ∫₀^(π/2) dθ/(1 + m sin²θ) = (π/2)/√(1 + m)  (for m > –1).
Here, m = t² so that
  J(t) = (π/2)/√(1 + t²).
Thus,
  I = 2 ∫₀¹ (π/2)/√(1 + t²) dt = π ∫₀¹ dt/√(1 + t²).

Step 6. Final t–Integral

We now have
  I = π ∫₀¹ dt/√(1 + t²).
This integral is elementary and can be computed by the substitution t = sinh u or by recalling that
  ∫ dt/√(1+t²) = asinh(t) = ln(t + √(1+t²)).
Evaluating from 0 to 1 gives:
  ∫₀¹ dt/√(1+t²) = asinh(1) – asinh(0) = ln(1 + √2) – 0 = ln(1+√2).
So finally,
  I = π ln(1+√2).

Step 7. Numerical Approximation

To 10 decimal places, note that
  ln(1+√2) ≈ ln(2.4142135624) ≈ 0.8813730000,
and therefore
  I ≈ π × 0.8813730000 ≈ 2.7690354657.

Thus, the exact answer is π ln(1+√2) and the numerical value is approximately 2.7690354657.

{"answer": "$\\pi \\ln(1+\\sqrt{2})$", "numerical_answer": "2.7690354657"}