Let's proceed step by step.

### 1. The Integral

\[
I = \int_{0}^{1} x^{-1/2}(1-x)^{-1/2} T_{4}\left(\sqrt{x(1-x)}\right)\, dx
\]

where \( T_4 \) is the Chebyshev polynomial of degree 4.

### 2. Find \( T_4(z) \)

Recall:
\[
T_n(z) = \cos(n\arccos z)
\]
For \( n=4 \):
\[
T_4(z) = 8z^4 - 8z^2 + 1
\]

Let \( z = \sqrt{x(1-x)} \):

\[
T_4(\sqrt{x(1-x)}) = 8[x(1-x)]^2 - 8[x(1-x)] + 1
\]
\[
= 8[x^2 - 2x^3 + x^4] - 8(x - x^2) + 1
\]
But it's best to keep as \( 8x^2(1-x)^2 - 8x(1-x) + 1 \).

### 3. Substitute and Expand

\[
I = \int_0^1 x^{-1/2}(1-x)^{-1/2}\left[8x^2(1-x)^2 - 8x(1-x) + 1\right] dx
\]
\[
= 8 \int_0^1 x^{-1/2}(1-x)^{-1/2} x^2(1-x)^2 dx - 8 \int_0^1 x^{-1/2}(1-x)^{-1/2} x(1-x) dx + \int_0^1 x^{-1/2}(1-x)^{-1/2} dx
\]
Let’s denote these as \( I_1, I_2, I_3 \):

\[
I_1 = \int_0^1 x^{-1/2} (1-x)^{-1/2} x^2 (1-x)^2 dx
\]
\[
= \int_0^1 x^{3/2 - 1} (1-x)^{3/2 - 1} dx
= \int_0^1 x^{3/2-1}(1-x)^{3/2-1}\, dx
= \int_0^1 x^{1.5-1}(1-x)^{1.5-1} dx
\]
\[
= \int_0^1 x^{1/2} (1-x)^{1/2} dx
\]

But more precisely, \( x^{-1/2} x^2 = x^{3/2} \), and \( (1-x)^{-1/2}(1-x)^2 = (1-x)^{3/2} \):

\[
I_1 = \int_0^1 x^{3/2}(1-x)^{3/2} dx
\]

Similarly:

\[
I_2 = \int_0^1 x^{-1/2}(1-x)^{-1/2} x(1-x) dx
\]
\[
= \int_0^1 x^{1/2}(1-x)^{1/2} dx
\]

and

\[
I_3 = \int_0^1 x^{-1/2}(1-x)^{-1/2} dx
\]

### 4. Express as Beta Functions

Recall:

\[
\int_0^1 x^{a-1}(1-x)^{b-1}dx = B(a, b) = \frac{\Gamma(a)\Gamma(b)}{\Gamma(a+b)}
\]

- \( I_1: x^{3/2}(1-x)^{3/2} \) → \( a = 5/2, b = 5/2 \)
- \( I_2: x^{1/2}(1-x)^{1/2} \) → \( a = 3/2, b = 3/2 \)
- \( I_3: x^{-1/2}(1-x)^{-1/2} \) → \( a = 1/2, b = 1/2 \)

So:

\[
I_1 = B\left(\frac{5}{2},\frac{5}{2}\right)
\]
\[
I_2 = B\left(\frac{3}{2},\frac{3}{2}\right)
\]
\[
I_3 = B\left(\frac{1}{2},\frac{1}{2}\right)
\]

Thus,
\[
I = 8B\left(\frac{5}{2},\frac{5}{2}\right) - 8B\left(\frac{3}{2},\frac{3}{2}\right) + B\left(\frac{1}{2},\frac{1}{2}\right)
\]

### 5. Write Beta in Gamma Functions

Recall:
\[
B(a, b) = \frac{\Gamma(a)\Gamma(b)}{\Gamma(a+b)}
\]
Also \( \Gamma(n+1) = n\Gamma(n) \).

#### Compute
- \(\Gamma(1/2) = \sqrt{\pi}\)
- \(\Gamma(3/2) = \frac{1}{2}\sqrt{\pi}\)
- \(\Gamma(5/2) = \frac{3}{4}\sqrt{\pi}\)

- \(\Gamma(1) = 1\)
- \(\Gamma(2) = 1!\)
- \(\Gamma(3) = 2!\)
- \(\Gamma(4) = 6\)
- \(\Gamma(5) = 24\)

Let’s compute:

##### \( B(5/2,5/2) \)
\[
B\left(\frac{5}{2},\frac{5}{2}\right) = \frac{\Gamma\left(\frac{5}{2}\right)^2}{\Gamma(5)}
\]
\[
\Gamma\left(\frac{5}{2}\right) = \frac{3}{4}\sqrt{\pi}
\]
\[
\Gamma(5) = 24
\]
So,
\[
B\left(\frac{5}{2},\frac{5}{2}\right) = \frac{\left(\frac{3}{4}\sqrt{\pi} \right)^2}{24} = \frac{9}{16}\pi \times \frac{1}{24} = \frac{9\pi}{384}
\]

##### \( B(3/2,3/2) \)
\[
B\left(\frac{3}{2},\frac{3}{2}\right) = \frac{\Gamma(3/2)^2}{\Gamma(3)}
\]
\[
\Gamma(3/2) = \frac{1}{2}\sqrt{\pi}
\]
\[
\Gamma(3) = 2
\]
\[
B\left(\frac{3}{2},\frac{3}{2}\right) = \frac{\left(\frac{1}{2}\sqrt{\pi}\right)^2}{2} = \frac{1}{4}\pi \times \frac{1}{2} = \frac{\pi}{8}
\]

##### \( B(1/2,1/2) \)
\[
B(1/2,1/2) = \frac{\Gamma(1/2)^2}{\Gamma(1)} = \pi
\]

### 6. Plug in Values

Now substitute back:

\[
I = 8 \times \frac{9\pi}{384} - 8 \times \frac{\pi}{8} + \pi
\]
\[
= \frac{72\pi}{384} - \pi + \pi
\]
Simplify:
\[
\frac{72}{384} = \frac{3}{16}
\]
So:
\[
I = \frac{3}{16}\pi
\]

### 7. Final Answers

#### **Exact Answer:**
\[
I = \frac{3}{16}\pi
\]

#### **Numerical Approximation:**
\[
I \approx \frac{3}{16} \times 3.141592653589793 \approx 0.5890486225
\]

### 8. JSON Output

```json
{"answer": "\\frac{3}{16}\\pi", "numerical_answer": "0.5890486225"}
```