<think>
Okay, let's see. I need to compute the definite integral from 0 to infinity of [1/(x(x² + 4))] arctan(x) dx. Hmm, that looks a bit tricky, but maybe I can break it down step by step.

First, let me write down the integral properly:

∫₀^∞ [arctan(x) / (x(x² + 4))] dx

Hmm, integrating from 0 to infinity. The integrand has arctan(x), which complicates things. Maybe integration by parts? Or perhaps substitution? Let me think.

I remember that sometimes when there's an arctan(x) term, differentiating under the integral sign might help. Alternatively, using substitution. Let me consider substitution first.

Wait, another approach: maybe express arctan(x) as an integral itself. Since arctan(x) = ∫₀^1 [x / (1 + x² t²)] dt. That's a way to represent arctan(x) as an integral. Then, swapping the order of integration. Let me try that.

So, substituting arctan(x) into the original integral:

∫₀^∞ [1/(x(x² + 4))] [∫₀^1 x / (1 + x² t²) dt] dx

Then, swapping the order of integration (Fubini's theorem), assuming convergence:

∫₀^1 ∫₀^∞ [1/(x(x² + 4)) * x / (1 + x² t²)] dx dt

Simplify the integrand:

The x in the numerator cancels with the x in the denominator, so we have:

∫₀^1 ∫₀^∞ [1 / ((x² + 4)(1 + x² t²))] dx dt

Hmm, so now we have a double integral. Let me focus on the inner integral over x. Let me denote the inner integral as I(t):

I(t) = ∫₀^∞ [1 / ((x² + 4)(1 + x² t²))] dx

This looks like a rational function of x². Maybe partial fractions? Or substitution. Let me use substitution. Let me set y = x², but maybe not. Alternatively, use substitution u = x². Let me see.

Alternatively, use partial fractions. Let me consider the integrand:

1 / [(x² + 4)(1 + t² x²)] = A/(x² + 4) + B/(1 + t² x²)

But wait, since the denominator factors are quadratic, maybe we can express this as (A x + B)/(x² + 4) + (C x + D)/(1 + t² x²), but since the numerator is 1, which is a constant, perhaps the decomposition is simpler.

Alternatively, use the method of partial fractions for rational functions. Let me write:

1 / [(x² + 4)(1 + t² x²)] = [A x + B]/(x² + 4) + [C x + D]/(1 + t² x²)

But since the numerator is 0 degree and denominator is 4th degree, but since the denominator factors into two quadratics, perhaps constants instead of linear terms. Wait, maybe:

Let me set 1 = A(1 + t² x²) + B(x² + 4). Wait, but that's not correct because the denominator is (x² +4)(1 + t² x²). So, the partial fraction decomposition would be:

1 / [(x² +4)(1 + t² x²)] = [A/(x² +4)] + [B/(1 + t² x²)]

Let me check. Let me set:

1 = A(1 + t² x²) + B(x² +4)

Then, expanding:

1 = A + A t² x² + B x² + 4B

Grouping terms:

1 = (A + 4B) + x²)(A t² + B)

Therefore, equating coefficients:

For x² term: A t² + B = 0

Constant term: A + 4B = 1

So, from the first equation: B = -A t²

Substitute into the second equation:

A + 4(-A t²) = 1 → A(1 -4 t²) =1 → A = 1/(1 -4 t²)

Then, B = - t²/(1 -4 t²)

Therefore, the partial fractions are:

1 / [(x² +4)(1 + t² x²)] = [1/(1 -4 t²)] [1/(x² +4) - t²/(1 + t² x²)]

Therefore, the inner integral I(t) becomes:

I(t) = ∫₀^∞ [1/(1 -4 t²)] [1/(x² +4) - t²/(1 + t² x²)] dx

Factor out 1/(1 -4 t²):

I(t) = 1/(1 -4 t²) [∫₀^∞ 1/(x² +4) dx - t² ∫₀^∞ 1/(1 + t² x²) dx ]

Compute each integral separately.

First integral: ∫₀^∞ 1/(x² +4) dx. The integral of 1/(x² + a²) dx from 0 to ∞ is π/(2a). So here a=2, so it's π/(2*2) = π/4.

Second integral: ∫₀^∞ 1/(1 + t² x²) dx. Let me set u = t x, so du = t dx, dx = du/t. Then the integral becomes ∫₀^∞ 1/(1 + u²) * du/t = (1/t) * [arctan(u)] from 0 to ∞ = (1/t)(π/2 -0) = π/(2t)

Therefore, substituting back into I(t):

I(t) = 1/(1 -4 t²) [π/4 - t² * π/(2t) ] = 1/(1 -4 t²) [π/4 - (π t)/2 ]

Simplify the expression inside the brackets:

π/4 - (π t)/2 = π(1/4 - t/2) = π( (1 - 2t)/4 )

Therefore:

I(t) = π/(1 -4 t²) * (1 -2t)/4 = π (1 -2t)/(4(1 -4 t²))

Factor denominator: 1 -4 t² = (1 -2t)(1 +2t)

So:

I(t) = π (1 -2t)/(4(1 -2t)(1 +2t)) ) = π/(4(1 +2t)) )

Cancel out (1 -2t) from numerator and denominator, assuming 1 -2t ≠0. But when t=1/2, the denominator becomes zero. However, in our original partial fractions, we had 1/(1 -4 t²), so t ≠ ±1/2. But in our case, t is from 0 to1, so t=1/2 is within the integration range. Hmm, but maybe when we did partial fractions, we assumed that 1 -4 t² ≠0. So, perhaps this approach is valid except at t=1/2, but maybe the integral is still convergent there. Let me check later.

But proceeding, after cancellation, we get:

I(t) = π/(4(1 +2t))

Therefore, the original double integral becomes:

∫₀^1 I(t) dt = ∫₀^1 π/(4(1 +2t)) dt

So, integrating with respect to t:

π/4 ∫₀^1 1/(1 +2t) dt

Let me compute the integral:

Let u =1 +2t, du =2 dt, so dt = du/2. When t=0, u=1; t=1, u=3.

Therefore:

π/4 * (1/2) ∫₁³ 1/u du = π/8 [ln u]₁³ = π/8 (ln3 - ln1) = π/8 ln3

Since ln1=0, so the integral is (π ln3)/8.

Therefore, the exact value of the original integral is π ln3 /8.

Now, let me check if this makes sense. Let me verify the steps again.

First, we expressed arctan(x) as an integral from 0 to1 of x/(1 +x² t²) dt. Then swapped the order of integration. Then, the inner integral was computed via partial fractions, leading to I(t) = π/(4(1 +2t)). Then integrating over t from 0 to1 gives (π/8) ln3. That seems correct.

Wait, but when t=1/2, the denominator 1 -4 t² becomes 1 -4*(1/4)=0, so there's a singularity at t=1/2. However, in the partial fraction decomposition, we had:

1 / [(x² +4)(1 + t² x²)] = [1/(1 -4 t²)] [1/(x² +4) - t²/(1 + t² x²)]

But when t=1/2, the denominator 1 -4*(1/4)=0, so the partial fraction approach breaks down here. However, in the integral over t from 0 to1, t=1/2 is a point in the integrand. But when we computed I(t), after simplification, we got I(t) = π/(4(1 +2t)), which is valid even at t=1/2? Wait, let's check.

If t=1/2, then the original integrand for I(t) becomes:

1 / [(x² +4)(1 + (1/4)x²)] = 1 / [(x² +4)(x²/4 +1)] = 1 / [(x² +4)( (x² +4)/4 ) ] = 4/(x² +4)^2

So, I(t=1/2) = ∫₀^∞ 4/(x² +4)^2 dx. Let's compute that.

Using substitution x = 2 tanθ, dx = 2 sec²θ dθ. Then x² +4 =4 tan²θ +4=4 sec²θ. So:

I(t=1/2) = ∫ 4/(4 sec²θ)^2 * 2 sec²θ dθ from θ=0 to θ=π/2

Simplify:

4/(16 sec⁴θ) *2 sec²θ dθ = (4*2)/(16) ∫ sec²θ / sec⁴θ dθ = (8/16) ∫ cos²θ dθ = (1/2) ∫ (1 + cos2θ)/2 dθ = (1/4)[θ + (sin2θ)/2] from 0 to π/2

Evaluating at π/2: (1/4)(π/2 +0) = π/8

At 0: 0. So total is π/8.

But according to our previous expression I(t) = π/(4(1 +2t)), when t=1/2, that would be π/(4*(1 +1))= π/8, which matches. So even though the partial fractions approach had a division by zero at t=1/2, the final expression for I(t) is valid even at t=1/2. Therefore, the result is correct.

Therefore, the original integral is indeed (π ln3)/8.

Now, let's compute the numerical approximation. The exact value is (π ln3)/8.

Compute π ≈ 3.1415926536

ln3 ≈ 1.0986122887

Multiply them: 3.1415926536 * 1.0986122887 ≈ 3.1415926536 *1.0986122887

Let me compute this:

First, 3 *1.0986 ≈3.2958

0.1415926536 *1.0986122887 ≈0.1415926536*1 ≈0.1415926536, 0.1415926536*0.0986122887≈0.013962

So total ≈0.1415926536 +0.013962≈0.155554

So total π*ln3≈3.2958 +0.155554≈3.451354

Then divide by 8: 3.451354 /8 ≈0.43141925

But let me compute more accurately using calculator:

π ≈3.141592653589793

ln3≈1.0986122886681098

Multiply: 3.141592653589793 *1.0986122886681098

Compute:

3 *1.0986122886681098 =3.2958368660043294

0.141592653589793 *1.0986122886681098 ≈

First, 0.1 *1.0986122886681098=0.10986122886681098

0.041592653589793 *1.0986122886681098 ≈

0.04 *1.0986122886681098=0.04394449154672439

0.001592653589793 *1.0986122886681098≈0.001749

So total ≈0.10986122886681098 +0.04394449154672439 +0.001749≈0.15555472041353537

So total π*ln3≈3.2958368660043294 +0.15555472041353537≈3.451391586417864

Divide by8: 3.451391586417864 /8≈0.431423948302233

Rounded to 10 decimal places: 0.4314239483

So the numerical approximation is approximately 0.4314239483.

Therefore, the exact answer is (π ln3)/8, and the numerical approximation is approximately 0.4314239483.
</think>

{"answer": "\\frac{\\pi \\ln 3}{8}", "numerical_answer": "0.4314239483"}