Given:

\[
I = \int_0^\infty \frac{\{x\}^{\lceil x\rceil}}{1+\lceil x\rceil}\, dx.
\]

Letâ€™s proceed step by step.

---

**Step 1: Rewrite the Integral Using Integer Intervals**

Over the interval \( [n, n+1) \), \( \lceil x \rceil = n+1 \) and \( \{x\} = x - n \), for any integer \( n \geq 0 \).

So split:

\[
I = \sum_{n=0}^\infty \int_n^{n+1} \frac{(x-n)^{n+1}}{1 + (n+1)} dx
\]
\[
= \sum_{n=0}^\infty \int_{x=n}^{n+1} \frac{(x-n)^{n+1}}{n+2} dx
\]

Let \( t = x - n \implies dx = dt,\, t \in [0,1) \):

\[
= \sum_{n=0}^\infty \frac{1}{n+2} \int_{t=0}^1 t^{n+1} dt
\]

---

**Step 2: Perform the \( t \) Integral**

\[
\int_0^1 t^{n+1} dt = \left[ \frac{t^{n+2}}{n+2} \right]_0^1 = \frac{1}{n+2}
\]

So each term is:

\[
\frac{1}{n+2} \times \frac{1}{n+2} = \frac{1}{(n+2)^2}
\]

Thus,

\[
I = \sum_{n=0}^\infty \frac{1}{(n+2)^2}
\]
\[
= \sum_{k=2}^\infty \frac{1}{k^2}
\]

---

**Step 3: Summing the Series**

The sum \( \sum_{k=1}^\infty \frac{1}{k^2} = \zeta(2) = \frac{\pi^2}{6} \).

So,

\[
\sum_{k=2}^\infty \frac{1}{k^2} = \zeta(2) - 1 = \frac{\pi^2}{6} - 1
\]

So,

\[
I = \frac{\pi^2}{6} - 1
\]

---

**Step 4: Numerical Approximation**

\[
\frac{\pi^2}{6} \approx \frac{9.8696044011}{6} \approx 1.644934068
\]
\[
I \approx 1.644934068 - 1 = 0.644934068
\]

Rounded to 10 decimal places:

\[
I \approx 0.6449340680
\]

---

**Final Answer (JSON format):**

```json
{"answer": "\\frac{\\pi^2}{6} - 1", "numerical_answer": "0.6449340680"}
```