To evaluate the definite integral:

$$
\int_0^2 x^{1/4}(2 - x)^{-1/4} \cosh\left(\sqrt[4]{x(2 - x)}\right) \, dx
$$

we proceed through a series of carefully chosen substitutions and simplifications.

---

### **Step 1: Substitution and Simplification**

Let us define:

$$
t = \sqrt[4]{x(2 - x)} \quad \Rightarrow \quad t^4 = x(2 - x)
$$

This substitution simplifies the integrand significantly. Solving for $ x $ in terms of $ t $, we find that $ x $ and $ 2 - x $ are symmetric around 1, and the integral can be expressed in terms of $ t $ over the interval $ [0, 1] $.

After applying the substitution and simplifying, the integral becomes:

$$
I = 2\sqrt{2} \int_0^1 \frac{t^2}{\sqrt{1 - t^2}} \cosh(t) \, dt
$$

This is a key transformation that allows us to work with a more manageable integrand.

---

### **Step 2: Further Substitution and Integration**

We now perform a change of variable:

$$
\phi = \arcsin(t) \quad \Rightarrow \quad t = \sin\phi, \quad dt = \cos\phi \, d\phi
$$

This transforms the integral into:

$$
I = 2\sqrt{2} \int_0^{\pi/2} \sin^2\phi \cosh(\sin\phi) \, d\phi
$$

This integral can be evaluated using known results from special functions or via integration by parts.

---

### **Step 3: Integration by Parts**

Let us now evaluate:

$$
J = \int_0^{\pi/2} \sin^2\phi \cosh(\sin\phi) \, d\phi
$$

We apply integration by parts with:

- $ u = \sin\phi \Rightarrow du = \cos\phi \, d\phi $
- $ dv = \sin\phi \cosh(\sin\phi) \, d\phi \Rightarrow v = \cosh(\sin\phi) $

Then:

$$
J = \left[ \sin\phi \cosh(\sin\phi) \right]_0^{\pi/2} - \int_0^{\pi/2} \cosh(\sin\phi) \cos\phi \, d\phi
$$

Evaluating the boundary term:

$$
\sin\left(\frac{\pi}{2}\right) \cosh(1) = 1 \cdot \cosh(1), \quad \sin(0) \cosh(0) = 0
$$

So the boundary term is $ \cosh(1) $.

Now evaluate the remaining integral:

$$
\int_0^{\pi/2} \cosh(\sin\phi) \cos\phi \, d\phi
$$

Let $ u = \sin\phi \Rightarrow du = \cos\phi \, d\phi $, and the integral becomes:

$$
\int_0^1 \cosh(u) \, du = \sinh(1)
$$

Thus:

$$
J = \cosh(1) - \sinh(1) = \frac{e + e^{-1}}{2} - \frac{e - e^{-1}}{2} = \frac{2e^{-1}}{2} = \frac{1}{e}
$$

---

### **Step 4: Final Result**

Now that we have:

$$
J = \frac{1}{e}
$$

We substitute back into the expression for $ I $:

$$
I = 2\sqrt{2} \cdot J = \frac{2\sqrt{2}}{e}
$$

---

### **Step 5: Numerical Approximation**

Using the known value $ e \approx 2.718281828459045 $, we compute:

$$
\frac{2\sqrt{2}}{e} \approx \frac{2 \cdot 1.41421356237}{2.718281828459045} \approx \frac{2.82842712474}{2.718281828459045} \approx 1.0