We wish to evaluate

  I = ∫₀¹ (x − 1)/((x + 1) ln x) dx.

A fruitful method is to introduce a parameter a and consider the more general integral

  I(a) = ∫₀¹ (xᵃ − 1)/((x + 1) ln x) dx.

Note that for a = 1 we recover our original integral: I(1) = I, and for a = 0 we have I(0) = 0 (since x⁰ − 1 = 0).

Step 1. Differentiate with respect to a under the integral sign. Differentiating I(a) with respect to a gives
  I′(a) = d/da ∫₀¹ (xᵃ − 1)/((x+1) ln x) dx
      = ∫₀¹ d/da [(xᵃ − 1)/(ln x)] · (1/(x+1)) dx.
Since the derivative of xᵃ is xᵃ ln x (and the derivative of the constant –1 is 0), we obtain
  d/da [(xᵃ − 1)/(ln x)] = xᵃ.
Thus,
  I′(a) = ∫₀¹ xᵃ/(x+1) dx.

Step 2. Express I′(a) as a series. For x in (0,1] we can expand
  1/(x+1) = Σₙ₌₀∞ (−1)ⁿ xⁿ.
Then
  I′(a) = ∫₀¹ xᵃ Σₙ₌₀∞ (−1)ⁿ xⁿ dx
      = Σₙ₌₀∞ (−1)ⁿ ∫₀¹ x^(a+n) dx
      = Σₙ₌₀∞ (−1)ⁿ/(a+n+1).
(The interchange of sum and integral is justified for 0 ≤ x ≤ 1.)

Step 3. Integrate with respect to a. Notice that
  I(a) = ∫₀ᵃ I′(t) dt = Σₙ₌₀∞ (−1)ⁿ ∫₀ᵃ dt/(t+n+1)
      = Σₙ₌₀∞ (−1)ⁿ ln((a+n+1)/(n+1)),
where we have used
  ∫₀ᵃ dt/(t+n+1) = ln((a+n+1)/(n+1)).
Since I(0) = 0, there is no constant of integration.

For a = 1 the result becomes
  I = I(1) = Σₙ₌₀∞ (−1)ⁿ ln((n+2)/(n+1))
      = Σₙ₌₀∞ (−1)ⁿ [ln(n+2) − ln(n+1)].

Step 4. Recognize a telescoping structure. Write the partial sum
  S_N = Σₙ₌₀ᴺ (−1)ⁿ [ln(n+2) − ln(n+1)]
     = Σₙ₌₀ᴺ (−1)ⁿ ln(n+2) − Σₙ₌₀ᴺ (−1)ⁿ ln(n+1).
Shift the index in the second sum by writing m = n + 1:
  Σₙ₌₀ᴺ (−1)ⁿ ln(n+1) = Σₘ₌₁ᴺ₊₁ (−1)^(m−1) ln m.
Thus,
  S_N = Σₘ₌₁ᴺ₊₁ (−1)^(m−1)[ln(m+1) − ln m] = Σₘ₌₁ᴺ₊₁ (−1)^(m−1) ln((m+1)/m).

This can be written as the logarithm of a product:
  S_N = ln (∏ₘ₌₁ᴺ₊₁ ((m+1)/m)^( (−1)^(m−1) )).
Denote
  P_N = ∏ₘ₌₁ᴺ₊₁ ((m+1)/m)^( (−1)^(m−1) ).
Let us write out the first few factors:
  For m = 1: ((2)/1)^(+1) = 2.
  For m = 2: ((3)/2)^(−1) = 2/3.
  For m = 3: ((4)/3)^(+1) = 4/3.
  For m = 4: ((5)/4)^(−1) = 4/5.
Thus,
  P_N = 2 · (2/3) · (4/3) · (4/5) · ⋯.

Grouping the factors for odd and even m leads to a product representation:
  P = limₙ→∞ P_N = [∏ₖ₌₀∞ (2k+2)/(2k+1)] / [∏ₖ₌₀∞ (2k+3)/(2k+2)]
    = ∏ₖ₌₀∞ [(2k+2)²/((2k+1)(2k+3))].

Rewriting the factors as
  (2k+2)² = 4(k+1)²  and (2k+1)(2k+3) = 4(k+1)² − 1,
we recognize that the infinite product
  ∏ₖ₌₀∞ [4(k+1)²/(4(k+1)² − 1)]
is known to be equal to π/2 (this is essentially the Wallis product).

Thus, one obtains
  P = π/2  and hence S = ln(P) = ln(π/2).

Therefore, the original integral is
  I = ln(π/2).

Step 5. A numerical approximation. Using
  ln(π/2) = ln(π) − ln(2),
with ln(π) ≈ 1.14472988585 and ln2 ≈ 0.69314718056, we have
  I ≈ 1.14472988585 − 0.69314718056 = 0.45158270529.
Rounded to 10 decimal places, this is 0.4515827053.

Final Answer in JSON Format:
{"answer": "\\ln\\frac{\\pi}{2}", "numerical_answer": "0.4515827053"}