<think>
Okay, let's tackle this integral: ∫₀¹ x arcsin(x) arccos(x) dx. Hmm, integrating a product of inverse trigonometric functions multiplied by x. That seems a bit tricky. Let me think about possible strategies.

First, I remember that arcsin(x) and arccos(x) are related. Specifically, arcsin(x) + arccos(x) = π/2. Maybe I can simplify the product using this identity. Let me try that.

Let’s set θ = arcsin(x), so arccos(x) would be π/2 - θ. Then the product arcsin(x) arccos(x) becomes θ(π/2 - θ). So the integral becomes ∫ x θ (π/2 - θ) dx. But x is sinθ, since θ = arcsin(x). So maybe substitution here. Let me check.

Wait, substitution might complicate things. Alternatively, maybe integration by parts. The integrand is x times arcsin(x) times arccos(x). Let me denote u = arcsin(x) arccos(x), and dv = x dx. But integration by parts might not be straightforward here because u is a product of two functions. Alternatively, maybe expand the product first using the identity.

Since arcsin(x) + arccos(x) = π/2, then arccos(x) = π/2 - arcsin(x). So the product arcsin(x)arccos(x) = arcsin(x)(π/2 - arcsin(x)) = (π/2) arcsin(x) - (arcsin(x))². So the integral becomes ∫₀¹ x [ (π/2) arcsin(x) - (arcsin(x))² ] dx. That splits into two integrals: (π/2) ∫₀¹ x arcsin(x) dx - ∫₀¹ x (arcsin(x))² dx. Maybe these are easier to handle.

Let me handle them one by one. First, compute I1 = ∫ x arcsin(x) dx. Then compute I2 = ∫ x (arcsin(x))² dx. Then the original integral is (π/2) I1 - I2.

Starting with I1: ∫ x arcsin(x) dx. Let's use integration by parts. Let u = arcsin(x), dv = x dx. Then du = 1/√(1 - x²) dx, and v = x²/2. So integration by parts gives uv - ∫ v du = (x²/2) arcsin(x) - ∫ (x²/2)(1/√(1 - x²)) dx. Simplify the integral: (1/2) ∫ x² / √(1 - x²) dx.

To compute ∫ x² / √(1 - x²) dx, maybe use substitution. Let x = sinθ, so dx = cosθ dθ, and √(1 - x²) = cosθ. Then the integral becomes ∫ sin²θ / cosθ * cosθ dθ = ∫ sin²θ dθ. Which is ∫ (1 - cos2θ)/2 dθ = (θ/2 - sin2θ/4) + C. Reverting back to x: θ = arcsin(x), so (arcsin(x)/2 - (sin(2 arcsin(x)))/4). But sin(2θ) = 2 sinθ cosθ = 2x√(1 - x²). So the integral becomes (arcsin(x)/2 - (x√(1 - x²))/2 ) + C. Therefore, the integral I1 is (x²/2) arcsin(x) - (1/2)(arcsin(x)/2 - (x√(1 - x²))/2 ) + C. Wait, let me check:

Wait, the integral after integration by parts was (x²/2) arcsin(x) - (1/2) ∫ x² / √(1 - x²) dx. Then we computed ∫ x² / √(1 - x²) dx as (arcsin(x)/2 - x√(1 - x²)/2 ). So substituting back, I1 becomes (x²/2) arcsin(x) - (1/2)(arcsin(x)/2 - x√(1 - x²)/2 ) + C. Simplify: (x²/2) arcsin(x) - arcsin(x)/4 + x√(1 - x²)/4 + C. So evaluated from 0 to 1.

At x=1: arcsin(1) = π/2, x²=1, so first term: (1/2)(π/2) = π/4. Second term: -π/8. Third term: 1*0/4 = 0. So total at 1: π/4 - π/8 = π/8.

At x=0: All terms are 0. So I1 from 0 to1 is π/8.

Now, moving to I2 = ∫₀¹ x (arcsin(x))² dx. Hmm, this seems more complicated. Let's use integration by parts again. Let u = (arcsin(x))², dv = x dx. Then du = 2 arcsin(x) * (1/√(1 - x²)) dx, and v = x²/2. So integration by parts gives uv|₀¹ - ∫ v du = (x²/2)(arcsin(x))² evaluated from 0 to1 - ∫ (x²/2)(2 arcsin(x)/√(1 - x²)) dx. Simplify: [ (1/2)(π/2)² - 0 ] - ∫ (x² arcsin(x))/√(1 - x²) dx. So that's π²/8 - ∫ x² arcsin(x)/√(1 - x²) dx.

Now, need to compute the integral J = ∫ x² arcsin(x)/√(1 - x²) dx. Let me consider substitution. Let t = arcsin(x), so x = sin t, dx = cos t dt, and √(1 - x²) = cos t. Then J becomes ∫ (sin² t) * t / cos t * cos t dt = ∫ t sin² t dt. So J = ∫ t sin² t dt. Let's compute this integral.

Use the identity sin² t = (1 - cos2t)/2. So J = ∫ t (1 - cos2t)/2 dt = (1/2) ∫ t dt - (1/2) ∫ t cos2t dt. The first integral is (1/2)(t²/2) = t²/4. The second integral: ∫ t cos2t dt. Integration by parts. Let u = t, dv = cos2t dt. Then du = dt, v = (1/2) sin2t. So ∫ t cos2t dt = (t/2) sin2t - ∫ (1/2) sin2t dt = (t/2) sin2t + (1/4) cos2t + C. So putting back into J: J = t²/4 - (1/2)[ (t/2) sin2t + (1/4) cos2t ] + C = t²/4 - t sin2t/4 - cos2t/8 + C.

Now, revert back to x. Since t = arcsin(x), and sin2t = 2 sin t cos t = 2x√(1 - x²). Also, cos2t = 1 - 2 sin² t = 1 - 2x². So substituting:

J = (arcsin(x))² /4 - (arcsin(x) * 2x√(1 - x²))/4 - (1 - 2x²)/8 + C. Simplify:

J = (arcsin(x))² /4 - (x arcsin(x) √(1 - x²))/2 - (1 - 2x²)/8 + C.

Therefore, going back to the expression for I2:

I2 = π²/8 - J evaluated from 0 to1. So:

I2 = π²/8 - [ (arcsin(1))² /4 - (1 * arcsin(1) * 0)/2 - (1 - 2*1)^2/8 ] + [ same at 0 ].

Wait, let's compute the limits. At x=1:

arcsin(1) = π/2, so first term: (π²/4)/4 = π²/16. Second term: 0. Third term: (1 - 2*1)/8 = (-1)/8. So J at 1: π²/16 - 0 - (-1)/8 = π²/16 + 1/8.

At x=0:

arcsin(0) = 0, so first term: 0. Second term: 0. Third term: (1 - 0)/8 = 1/8. So J at 0: 0 - 0 - 1/8 = -1/8.

Therefore, J evaluated from 0 to1 is [π²/16 +1/8] - (-1/8) = π²/16 +1/8 +1/8 = π²/16 + 1/4.

Thus, I2 = π²/8 - (π²/16 + 1/4) = π²/8 - π²/16 -1/4 = π²/16 -1/4.

So putting it all together, the original integral is (π/2)*I1 - I2 = (π/2)*(π/8) - (π²/16 -1/4) = π²/16 - π²/16 +1/4 = 1/4. Wait, that can't be right. Wait, let's check:

Wait, (π/2)*I1 is (π/2)*(π/8) = π²/16.

Then subtract I2: π²/16 - (π²/16 -1/4) = π²/16 - π²/16 +1/4 = 1/4. So the integral equals 1/4? That seems surprisingly simple. Let me verify.

Wait, but 1/4 is a very clean result. Let me check the steps again.

First, I1 was computed as π/8. Then I2 was π²/16 -1/4. Then the original integral is (π/2)(π/8) - (π²/16 -1/4) = π²/16 - π²/16 +1/4 = 1/4. So yes, the integral is 1/4. Hmm, that seems correct. Let me check with a numerical approximation.

Alternatively, let's compute the integral from 0 to1 of x arcsin(x) arccos(x) dx numerically. Let's approximate it. For example, using substitution x=0.5, the integrand is 0.5 * arcsin(0.5) * arccos(0.5). arcsin(0.5)=π/6≈0.5235987756, arccos(0.5)=π/3≈1.0471975512. So product is ≈0.5 *0.5235987756 *1.0471975512≈0.5*0.548311≈0.274155. But integrating from 0 to1, the function starts at 0, peaks somewhere, and ends at 0 (since at x=1, arccos(1)=0). The integral being 0.25 seems plausible. Let me check with another point. At x=1/√2≈0.7071, arcsin(x)=π/4, arccos(x)=π/4. So integrand is (1/√2)*(π/4)^2≈0.7071*(0.61685)≈0.436. The area under the curve from 0 to1 might sum up to 0.25. Let me compute a rough numerical approximation.

Alternatively, use substitution. Let me compute the integral numerically. Let's approximate using, say, Simpson's rule with n=4 intervals. Divide [0,1] into 4 intervals: h=0.25. Points: 0, 0.25, 0.5, 0.75, 1.

Compute f(x) at these points:

At x=0: 0*arcsin(0)*arccos(0)=0.

At x=0.25: 0.25 * arcsin(0.25) * arccos(0.25). arcsin(0.25)≈0.2527 radians, arccos(0.25)≈1.3181 radians. So product≈0.25*0.2527*1.3181≈0.25*0.333≈0.0833.

At x=0.5: as before≈0.274155.

At x=0.75: x=0.75, arcsin(0.75)≈0.84806, arccos(0.75)≈0.7227 radians. Product:0.75*0.84806*0.7227≈0.75*0.6127≈0.4595.

At x=1: 0.

Simpson's rule: (h/3)[f(0) +4(f(0.25)+f(0.75)) +2(f(0.5)) +f(1)] = (0.25/3)[0 +4*(0.0833+0.4595) +2*0.274155 +0] ≈ (0.083333)[4*(0.5428) +0.54831] ≈0.083333*(2.1712 +0.54831)=0.083333*2.7195≈0.2266. Which is lower than 0.25, but Simpson's rule with n=4 is not very accurate. Let's try with n=2 (which is worse). But maybe the exact answer is indeed 1/4. Let's check with higher n. Alternatively, accept that the analytical result is 1/4, and the numerical approximation would be 0.25. But let's compute it more accurately.

Alternatively, use substitution. Let me compute the exact value again. Wait, the steps led to 1/4. Let me check the I2 calculation again.

I2 = π²/8 - [J evaluated from 0 to1]. J evaluated from 0 to1 was π²/16 +1/4. So I2 = π²/8 - (π²/16 +1/4) = π²/16 -1/4. Then original integral is (π/2)*I1 - I2 = (π/2)*(π/8) - (π²/16 -1/4) = π²/16 - π²/16 +1/4 = 1/4. So the exact answer is 1/4. Therefore, the numerical approximation is 0.25. So the answer is {"answer": "\dfrac{1}{4}", "numerical_answer": 0.25}. But let me confirm once more.

Wait, maybe there's a mistake in the calculation of J. Let me recheck J.

J = ∫ x² arcsin(x)/√(1 - x²) dx. After substitution t=arcsin(x), becomes ∫ t sin² t dt. Then expanding sin² t as (1 - cos2t)/2, so J = (1/2) ∫ t dt - (1/2) ∫ t cos2t dt. The first integral is t²/4. The second integral, after integration by parts, is (1/2)[ (t/2) sin2t + (1/4) cos2t ].

Wait, the integral of t cos2t dt is (t/2) sin2t - ∫ (1/2) sin2t dt = (t/2) sin2t + (1/4) cos2t. So the second term is - (1/2) [ (t/2) sin2t + (1/4) cos2t ].

So J = t²/4 - (1/2)(t/2 sin2t + 1/4 cos2t) + C = t²/4 - t sin2t/4 - cos2t/8 + C. Correct.

Then substituting back t=arcsin(x), sin2t=2x√(1 -x²), cos2t=1-2x². So J becomes (arcsin(x))²/4 - (arcsin(x)*2x√(1 -x²))/4 - (1 -2x²)/8 + C. Correct.

Evaluating from 0 to1:

At x=1: arcsin(1)=π/2, so first term: (π²/4)/4=π²/16. Second term: (π/2 * 2*1*0)/4=0. Third term: -(1 -2*1)/8= -(-1)/8=1/8. So total at 1: π²/16 +1/8.

At x=0: arcsin(0)=0, so first term:0. Second term:0. Third term: -(1 -0)/8= -1/8. So total at 0: -1/8.

Thus, J from 0 to1 is (π²/16 +1/8) - (-1/8) = π²/16 +1/4. Therefore, I2=π²/8 - (π²/16 +1/4)= π²/16 -1/4. Then original integral is (π/2)(π/8) - (π²/16 -1/4)= π²/16 -π²/16 +1/4=1/4. Yes, so exact answer is 1/4. Numerical approximation is 0.25. So the JSON should be {"answer": "\dfrac{1}{4}", "numerical_answer": 0.2500000000}.
</think>

{"answer": "\dfrac{1}{4}", "numerical_answer": 0.2500000000}