Let's compute the definite integral:
\[
I = \int_0^1 \frac{1}{x} \arccos x\, (\arcsin x)^2 \,dx
\]

**Step 1: Substitution**

Let \( x = \sin \theta \), so as \( x \) goes from \( 0 \) to \( 1 \), \( \theta \) goes from \( 0 \) to \( \frac{\pi}{2} \).

Recall that \(\arccos x = \arccos(\sin\theta) = \frac{\pi}{2} - \theta\) and \(\arcsin x = \arcsin(\sin\theta) = \theta\).

Compute derivatives:
\[
dx = \cos \theta\, d\theta
\]
\[
x = \sin\theta \implies \frac{1}{x} = \frac{1}{\sin\theta}
\]

So, substituting,
\[
I = \int_{\theta=0}^{\pi/2} \frac{1}{\sin\theta} \arccos(\sin\theta) (\arcsin(\sin\theta))^2 \cos\theta\, d\theta
\]
\[
= \int_0^{\pi/2} \frac{1}{\sin\theta} \left(\frac{\pi}{2} - \theta \right) \theta^2 \cos\theta d\theta
\]
\[
= \int_0^{\pi/2} \left(\frac{\pi}{2} - \theta\right) \theta^2 \frac{\cos\theta}{\sin\theta} d\theta
\]
\[
= \int_0^{\pi/2} \left(\frac{\pi}{2} - \theta\right) \theta^2 \cot\theta d\theta
\]

**Step 2: Expand and Separate Integrals**

Let’s expand the integrand:
\[
I = \frac{\pi}{2} \int_0^{\pi/2} \theta^2 \cot\theta d\theta - \int_0^{\pi/2} \theta^3 \cot\theta d\theta
\]
Let’s denote:
\[
I_1 = \int_0^{\pi/2} \theta^2 \cot\theta\, d\theta,\qquad I_2 = \int_0^{\pi/2} \theta^3 \cot\theta\, d\theta
\]
So,
\[
I = \frac{\pi}{2} I_1 - I_2
\]

**Step 3: Compute \( I_1 \)**

Integrate by parts:
Let \( u = \theta^2 \), \( dv = \cot\theta\, d\theta \),
then \( du = 2\theta d\theta \), \( v = \log\sin\theta \).

So,
\[
I_1 = \left. \theta^2 \log\sin\theta \right|_0^{\pi/2} - \int_0^{\pi/2} 2\theta \log\sin\theta d\theta
\]
As \(\theta\to 0\), \(\theta^2 \log\sin\theta \to 0\) (since \(\log\sin\theta \sim \log \theta\) and \(\theta^2\) dominates).

At \(\theta = \frac{\pi}{2}\), \(\log\sin\frac{\pi}{2}=0\), so boundary term vanishes.

Thus,
\[
I_1 = -2 \int_0^{\pi/2} \theta \log\sin\theta d\theta
\]

Let’s use the known integral:
\[
J_1 = \int_0^{\pi/2} \theta \log\sin\theta d\theta
\]

This is a classic integral. Recall:
\[
\int_0^{\pi/2} x \log \sin x\, dx = \frac{1}{2} \left( \frac{\pi}{2} \right)^2 \log 2 - \frac{7}{16} \zeta(3)
\]

Proof:
\[
\int_0^{\pi/2} x \log\sin x\, dx = \frac{\pi^2}{8} \log 2 - \frac{7}{16} \zeta(3)
\]

So,
\[
I_1 = -2 J_1 = -2 \left( \frac{\pi^2}{8} \log 2 - \frac{7}{16} \zeta(3) \right )
= -\frac{\pi^2}{4} \log 2 + \frac{7}{8}\zeta(3)
\]

**Step 4: Compute \( I_2 \)**

Integrate by parts:
Let \( u = \theta^3 \), \( dv = \cot\theta\, d\theta \),
then \( du = 3\theta^2 d\theta \), \( v = \log\sin\theta \).
\[
I_2 = \left. \theta^3 \log\sin\theta \right|_0^{\pi/2} - \int_0^{\pi/2} 3\theta^2 \log\sin\theta d\theta
\]
Again, boundary vanishes.

So,
\[
I_2 = -3 \int_0^{\pi/2} \theta^2 \log\sin\theta d\theta
\]

Let’s let \( J_2 = \int_0^{\pi/2} \theta^2 \log\sin\theta d\theta \).

This is a known result (see Gradshteyn & Ryzhik 4.231.3, or via series expansion):

It can be shown that:
\[
J_2 = \frac{\pi^3}{24} \log 2 - \frac{93}{256} \zeta(4)
\]
But let's derive it for completeness.

Expand \(\log\sin\theta\) in Fourier series:
\[
\log\sin\theta = -\log 2 - \sum_{k=1}^{\infty} \frac{\cos 2k\theta}{k}
\]
So,
\[
J_2 = \int_0^{\pi/2} \theta^2 \log\sin\theta d\theta = -\log 2 \int_0^{\pi/2} \theta^2 d\theta - \sum_{k=1}^{\infty} \frac{1}{k} \int_0^{\pi/2} \theta^2 \cos 2k\theta d\theta
\]
Compute:
\[
\int_0^{\pi/2} \theta^2 d\theta = \frac{(\pi/2)^3}{3} = \frac{\pi^3}{24}
\]
Next,
\[
\int_0^{\pi/2} \theta^2 \cos 2k\theta d\theta
\]
Let’s recall:
\[
\int_0^a x^n \cos bx dx = \text{(integral table)}
\]
Set \( n=2, b=2k, a=\frac{\pi}{2} \):

Let’s compute:

By parts twice or use the known result:
\[
\int_0^A x^2 \cos \alpha x dx = \frac{2\alpha A \sin\alpha A + ( \alpha^2 A^2 - 2 )\cos\alpha A + 2 }{\alpha^3}
\]

Set \( A = \frac{\pi}{2}, \alpha = 2k \):

\[
\int_0^{\pi/2} \theta^2 \cos(2k\theta) d\theta
= \left. \frac{2(2k)\theta \sin(2k\theta) + ((2k)^2 \theta^2 - 2)\cos(2k\theta) + 2}{(2k)^3} \right|_0^{\pi/2}
\]

Calculate:

At \(\theta=0\), both terms vanish except last +2:

- \( \sin(0) = 0 \)
- \( \theta^2 = 0 \), \( \cos(0) = 1 \)
- So, get \( -2 \times 1 + 2 = 0 \).

At \( \theta = \frac{\pi}{2} \):

Compute:

\[
2kA \sin(2kA) = 2k \cdot \frac{\pi}{2} \cdot \sin (2k \cdot \frac{\pi}{2}) = k\pi \sin (k\pi) = 0
\]
\[
(2k)^2 A^2 = 4k^2 \left( \frac{\pi}{2} \right)^2 = k^2 \pi^2
\]
\[
\cos(2kA) = \cos (k\pi) = (-1)^k
\]
So,
\[
(k^2 \pi^2 - 2) \cos(2kA) + 2 = (k^2\pi^2 - 2)(-1)^k + 2
\]

So overall,
\[
\int_0^{\pi/2} \theta^2 \cos(2k\theta) d\theta
= \frac{(k^2 \pi^2 - 2)(-1)^k + 2}{8k^3}
\]

So,
\[
J_2 = -\log 2 \cdot \frac{\pi^3}{24} - \sum_{k=1}^{\infty} \frac{1}{k} \cdot \frac{(k^2 \pi^2 - 2)(-1)^k + 2}{8k^3}
\]
\[
= -\log 2 \cdot \frac{\pi^3}{24} - \frac{1}{8} \sum_{k=1}^{\infty} \frac{(k^2 \pi^2 - 2)(-1)^k + 2}{k^4}
\]
\[
= -\frac{\pi^3}{24} \log 2 - \frac{1}{8} \left( \sum_{k=1}^\infty \frac{(k^2 \pi^2 - 2)(-1)^k}{k^4} + 2\sum_{k=1}^\infty \frac{1}{k^4} \right )
\]

Now, \(\sum_{k=1}^\infty \frac{1}{k^4} = \zeta(4) = \frac{\pi^4}{90}\)

\(\sum_{k=1}^\infty \frac{(-1)^k}{k^4} = -\frac{\pi^4}{90} + 2 \sum_{n=1}^\infty \frac{1}{(2n)^4} = -\frac{\pi^4}{90} + \frac{1}{16} \zeta(4)\)

But more directly, \( \sum_{k=1}^\infty \frac{(-1)^k}{k^4} = -\frac{7}{8}\zeta(4) \).

Additionally, \(\sum_{k=1}^\infty \frac{(-1)^k k^2}{k^4} = \sum_{k=1}^\infty \frac{(-1)^k}{k^2} = -\frac{\pi^2}{12}\).

Therefore,

\[
\sum_{k=1}^\infty \frac{(k^2 \pi^2 - 2)(-1)^k}{k^4} = \pi^2 \sum_{k=1}^\infty \frac{(-1)^k}{k^2} - 2 \sum_{k=1}^\infty \frac{(-1)^k}{k^4} = -\frac{\pi^4}{12} + \frac{7}{4} \zeta(4)
\]

Putting it all together,
\[
J_2 = -\frac{\pi^3}{24} \log 2 - \frac{1}{8} \left( -\frac{\pi^4}{12} + \frac{7}{4}\zeta(4) + 2\zeta(4) \right )
\]
\[
= -\frac{\pi^3}{24} \log 2 - \frac{1}{8} \left( -\frac{\pi^4}{12} + \frac{15}{4}\zeta(4) \right )
\]
\[
= -\frac{\pi^3}{24} \log 2 + \frac{\pi^4}{96} - \frac{15}{32}\zeta(4)
\]

Therefore,
\[
I_2 = -3J_2 = \frac{\pi^3}{8} \log 2 - \frac{\pi^4}{32} + \frac{45}{32}\zeta(4)
\]

**Step 5: Put Everything Together**

Recall:
\[
I = \frac{\pi}{2} I_1 - I_2
\]
Plug in the values computed:

\[
I_1 = -\frac{\pi^2}{4} \log 2 + \frac{7}{8}\zeta(3)
\]
\[
I_2 = \frac{\pi^3}{8} \log 2 - \frac{\pi^4}{32} + \frac{45}{32}\zeta(4)
\]
\[
I = \frac{\pi}{2} \left( -\frac{\pi^2}{4}\log 2 + \frac{7}{8}\zeta(3) \right ) - \left( \frac{\pi^3}{8} \log 2 - \frac{\pi^4}{32} + \frac{45}{32}\zeta(4) \right )
\]
\[
= -\frac{\pi^3}{8}\log 2 + \frac{7 \pi}{16}\zeta(3) - \frac{\pi^3}{8} \log 2 + \frac{\pi^4}{32} - \frac{45}{32}\zeta(4)
\]
\[
= -\frac{\pi^3}{4}\log 2 + \frac{7 \pi}{16}\zeta(3) + \frac{\pi^4}{32} - \frac{45}{32}\zeta(4)
\]

**Therefore, the exact value is:**
\[
\boxed{
I = -\frac{\pi^3}{4} \log 2 + \frac{7\pi}{16}\zeta(3) + \frac{\pi^4}{32} - \frac{45}{32}\zeta(4)
}
\]

---

**Step 6: Numerical Approximation**

Let’s compute numerically:

- \(\pi \approx 3.1415926536\)
- \(\zeta(3) \approx 1.2020569032\)
- \(\zeta(4) = \frac{\pi^4}{90} \approx 1.0823232330\)
- \(\log 2 \approx 0.6931471806\)

Compute:

- \(\frac{\pi^3}{4} \log 2 \approx \frac{(3.1415926536)^3}{4} \cdot 0.6931471806
= \frac{31.00627668}{4} \cdot 0.6931471806
= 7.751569172 \cdot 0.6931471806 \approx 5.374795321\)

- \( \frac{7\pi}{16}\zeta(3) \approx \frac{7 \cdot 3.1415926536}{16} \cdot 1.2020569032 = 1.3744467858 \cdot 1.2020569032 \approx 1.651380597 \)

- \(\frac{\pi^4}{32} \approx \frac{(3.1415926536)^4}{32} = \frac{97.4090910}{32} \approx 3.044034094\)

- \(\frac{45}{32} \zeta(4) \approx 1.40625 \times 1.0823232330 \approx 1.522941373\)

Now, combine:
\[
I = -5.374795321 + 1.651380597 + 3.044034094 - 1.522941373 = (1.651380597 + 3.044034094) - (5.374795321 + 1.522941373)
\]
\[
= 4.695414691 - 6.897736694 = -2.202322003
\]

So, to 10 decimal places:

\[
I \approx -2.2023220030
\]

---

**Final JSON Output:**
```json
{"answer": "-\\frac{\\pi^3}{4} \\log 2 + \\frac{7\\pi}{16} \\zeta(3) + \\frac{\\pi^4}{32} - \\frac{45}{32}\\zeta(4)", "numerical_answer": "-2.2023220030"}
```