We start with the integral

  I = ∫₁² (9x + 4)/(x⁵ + 3x² + x) dx.

Step 1. Factor the denominator:
  x⁵ + 3x² + x = x(x⁴ + 3x + 1).

So the integrand becomes
  (9x + 4) / [x (x⁴ + 3x + 1)].

Step 2. Write the integrand in partial fractions. Assume that
  (9x + 4) / [x (x⁴ + 3x + 1)] = A/x + (Bx³ + Cx² + Dx + E)/(x⁴ + 3x + 1).

Multiply both sides by the common denominator x(x⁴+3x+1) to obtain
  9x + 4 = A(x⁴ + 3x + 1) + x(Bx³ + Cx² + Dx + E).

Expanding the right-hand side gives:
  A*x⁴ + 3A*x + A + B*x⁴ + C*x³ + D*x² + E*x.

Now, equate the coefficients of like powers of x:
  x⁴: A + B = 0   ⟹  B = –A.
  x³: C = 0.
  x²: D = 0.
  x¹: 3A + E = 9   ⟹  E = 9 – 3A.
  x⁰: A = 4.

Thus, we have:
  A = 4,
  B = –4,
  C = D = 0,
  E = 9 – 12 = –3.

So the decomposition becomes:
  (9x + 4)/(x(x⁴+3x+1)) = 4/x + (–4x³ – 3)/(x⁴ + 3x + 1).

Step 3. Write the integral as the sum of two simpler integrals:
  I = ∫₁² 4/x dx + ∫₁² (–4x³ – 3)/(x⁴ + 3x + 1) dx.

The first one is straightforward:
  ∫₁² 4/x dx = 4 ln|x| evaluated from 1 to 2 = 4 ln2.

For the second integral, notice that the derivative of (x⁴ + 3x + 1) is 4x³ + 3. Thus,
  ∫ (–4x³ – 3)/(x⁴ + 3x + 1) dx = –∫ (4x³ + 3)/(x⁴ + 3x + 1) dx = – ln|x⁴ + 3x + 1| + constant.

Evaluating from 1 to 2:
  At x = 2: x⁴ + 3x + 1 = 16 + 6 + 1 = 23.
  At x = 1: x⁴ + 3x + 1 = 1 + 3 + 1 = 5.
  So the second part equals: – [ln(23) – ln(5)] = ln(5) – ln(23).

Step 4. Combine the two parts:
  I = 4 ln2 + [ln(5) – ln(23)] = 4 ln2 + ln(5/23).

We can combine the logarithms:
  4 ln2 = ln(2⁴) = ln16, so
  I = ln16 + ln(5/23) = ln(80/23).

Step 5. Numerical approximation:
  80/23 ≈ 3.4782608696  ⇒  ln(3.4782608696) ≈ 1.2465324187.

Thus, the exact answer is ln(80/23) and the numerical approximation (to 10 decimal places) is 1.2465324187.

{"answer": "\\ln\\left(\\frac{80}{23}\\right)", "numerical_answer": "1.2465324187"}