
To solve the definite integral \(\int_0^1 \arctan(x^2 - x + 1) \, dx\), we start by analyzing the argument of the arctangent function and using trigonometric identities.

### Step 1: Key Identity for \(\arctan(x^2 - x + 1)\)
First, we use the identity for the arctangent function: \(\arctan(z) = \frac{\pi}{2} - \arctan\left(\frac{1}{z}\right)\) for \(z > 0\). Since \(x^2 - x + 1 = \left(x - \frac{1}{2}\right)^2 + \frac{3}{4} > 0\) for all \(x\), we can apply this identity:
\[
\arctan(x^2 - x + 1) = \frac{\pi}{2} - \arctan\left(\frac{1}{x^2 - x + 1}\right).
\]

Next, we simplify \(\arctan\left(\frac{1}{x^2 - x + 1}\right)\). Using the tangent addition formula, we find that:
\[
\arctan(x) + \arctan(1 - x) = \arctan\left(\frac{1}{x^2 - x + 1}\right).
\]
This is verified by checking the tangent of the sum:
\[
\tan\left(\arctan(x) + \arctan(1 - x)\right) = \frac{x + (1 - x)}{1 - x(1 - x)} = \frac{1}{x^2 - x + 1}.
\]

Thus, we rewrite the original integrand:
\[
\arctan(x^2 - x + 1) = \frac{\pi}{2} - \arctan(x) - \arctan(1 - x).
\]

### Step 2: Integrate the Rewritten Expression
We now integrate term by term over \([0, 1]\):
\[
\int_0^1 \arctan(x^2 - x + 1) \, dx = \int_0^1 \left( \frac{\pi}{2} - \arctan(x) - \arctan(1 - x) \right) dx.
\]

#### Integral of \(\frac{\pi}{2}\)
\[
\int_0^1 \frac{\pi}{2} \, dx = \frac{\pi}{2} \cdot (1 - 0) = \frac{\pi}{2}.
\]

#### Integral of \(\arctan(x)\)
Using integration by parts (\(u = \arctan(x)\), \(dv = dx\)):
\[
\int \arctan(x) \, dx = x \arctan(x) - \frac{1}{2} \ln(1 + x^2) + C.
\]
Evaluating from \(0\) to \(1\):
\[
\left[ x \arctan(x) - \frac{1}{2} \ln(1 + x^2) \right]_0^1 = \left( 1 \cdot \frac{\pi}{4} - \frac{1}{2} \ln(2) \right) - \left( 0 - 0 \right) = \frac{\pi}{4} - \frac{1}{2} \ln(2).
\]

#### Integral of \(\arctan(1 - x)\)
Substitute \(t = 1 - x\) (so \(dt = -dx\)):
\[
\int_0^1 \arctan(1 - x) \, dx = \int_1^0 \arctan(t) (-dt) = \int_0^1 \arctan(t) \, dt = \frac{\pi}{4} - \frac{1}{2} \ln(2).
\]

### Step 3: Combine Results
Putting it all together:
\[
\int_0^1 \arctan(x^2 - x + 1) \, dx = \frac{\pi}{2} - \left( \frac{\pi}{4} - \frac{1}{2} \ln(2) \right) - \left( \frac{\pi}{4} - \frac{1}{2} \ln(2) \right) = \ln(2).
\]

### Numerical Approximation
The numerical value of \(\ln(2)\) is approximately \(0.69314718056\), rounded to 10 decimal places as \(0.6931471806\).

{"answer": "\(\ln 2\)", "numerical_answer": "0.6931471806"}