We wish to evaluate

  I = ∫₀² x^(–1/2) [1 + √(x(2 – x))]^(–3/2) dx.

Step 1. Change of variable

Let
  x = 2 sin²θ  with θ ∈ [0, π/2].
Then
  dx = 4 sinθ cosθ dθ  and x^(–1/2) = (2 sin²θ)^(–1/2) = 1/(√2 sinθ).

Also, note that
  √(x(2 – x)) = √[2 sin²θ · (2 – 2 sin²θ)]
          = √[4 sin²θ cos²θ] = 2 sinθ cosθ.

Substitute all these into I:

  I = ∫₀^(π/2) [1/(√2 sinθ)] · [1 + 2 sinθ cosθ]^(–3/2) · (4 sinθ cosθ dθ).

The factors of sinθ cancel:
  I = (4/(√2)) ∫₀^(π/2) cosθ [1 + 2 sinθ cosθ]^(–3/2) dθ
    = 2√2 ∫₀^(π/2) cosθ [1 + 2 sinθ cosθ]^(–3/2) dθ.

Step 2. Rewrite using a double‐angle identity

Recall that 2 sinθ cosθ = sin2θ, so the integral becomes

  I = 2√2 ∫₀^(π/2) cosθ (1 + sin2θ)^(–3/2) dθ.

Make the substitution t = 2θ. Then dθ = dt/2. When θ runs from 0 to π/2, t runs from 0 to π. Also, note that cosθ = cos(t/2); substituting we get

  I = 2√2 ∫₀^π cos(t/2) (1 + sin t)^(–3/2) (dt/2)
    = √2 ∫₀^π cos(t/2) (1 + sin t)^(–3/2) dt.

Step 3. Use the tangent half-angle substitution

Write cos(t/2) in a form that will be conveniently integrated by using the tangent half-angle substitution. Recall:

  u = tan(t/2),  so that dt = 2 du/(1 + u²),
  sin t = 2u/(1 + u²),  and cos t = (1 – u²)/(1 + u²).

In addition, use the half-angle formula for cosine:
  1 + cos t = 2 cos²(t/2)
  ⇒ cos(t/2) = √((1 + cos t)/2).

Now, express the factors in the integrand in terms of u.

First, we have
  1 + sin t = 1 + 2u/(1 + u²) = (1 + u² + 2u)/(1 + u²) = ((u + 1)²/(1 + u²)).
Thus,
  (1 + sin t)^(–3/2) = ((1 + u²)/(u + 1)²)^(3/2)
          = (1 + u²)^(3/2)/(u + 1)³.

Next, for cos(t/2), use the identity
  cos(t/2) = √((1 + cos t)/2).
But observe that
  1 + cos t = 1 + (1 – u²)/(1 + u²) = (2/(1 + u²)).
Thus,
  cos(t/2) = √[2/(1 + u²) · 1/2] = 1/√(1 + u²).

Finally, dt = 2 du/(1 + u²).

Now substitute into I:
  I = √2 ∫ (from u=tan0=0 to u=tan(π/2)=∞) [1/√(1+u²)] · [(1+u²)^(3/2)/(u+1)³] · [2 du/(1+u²)].
Simplify the integrand:
  The factors combine as:
   1/√(1+u²) · (1+u²)^(3/2) = (1+u²),
  then multiplying by 2/(1+u²) leaves a constant factor 2.
Thus,
  I = √2 · ∫₀^∞ [2/(u+1)³] du = 2√2 ∫₀^∞ du/(u+1)³.

Step 4. Evaluate the remaining simple integral

Make the substitution w = u+1 so that dw = du. When u = 0, w = 1; when u → ∞, w → ∞. Therefore,
  ∫₀^∞ du/(u+1)³ = ∫₁^∞ dw/w³.
This is a standard integral:
  ∫₁^∞ w^(–3) dw = [–1/(2 w²)]₁^∞ = (0 – (–1/2)) = 1/2.

Thus, the total value is
  I = 2√2 · (1/2) = √2.

Step 5. Final Answer

The exact value of the integral is √2.

The numerical approximation of √2 ≈ 1.4142135624 (to 10 decimal places).

The final answer in the required JSON format is:
{"answer": "$\\sqrt{2}$", "numerical_answer": "1.4142135624"}