Let's tackle the integral step by step:

\[
I = \int_{0}^{2} x^{-1/2} (2-x)^{-1/2} \left[1-0.5x(2-x)\right] \, dx
\]

Let's first expand the bracket:

\[
0.5 x(2-x) = x - 0.5x^2
\]
So,
\[
1 - 0.5x(2-x) = 1 - x + 0.5x^2
\]
Thus,
\[
I = \int_{0}^{2} x^{-1/2} (2-x)^{-1/2} \left(1 - x + 0.5x^2\right) dx
\]

Split into three integrals:
\[
I = \int_{0}^{2} x^{-1/2} (2-x)^{-1/2} dx - \int_{0}^{2} x^{1/2}(2-x)^{-1/2} dx + 0.5 \int_{0}^{2} x^{3/2} (2-x)^{-1/2} dx
\]

Let us compute each term separately.

---

### First Integral: \( I_1 = \int_{0}^{2} x^{-1/2} (2-x)^{-1/2} dx \)

Let \(x = 2 \sin^2 \theta\), \(dx = 4\sin\theta\cos\theta d\theta = 2\sin 2\theta\, d\theta\).
When \(x = 0\), \(\theta = 0\). When \(x = 2\), \(\theta = \pi/2\).

Calculate:

- \(x^{-1/2} = \left(2 \sin^2 \theta\right)^{-1/2} = (2)^{-1/2} (\sin \theta)^{-1}\)
- \(2-x = 2-2\sin^2\theta = 2\cos^2 \theta \implies (2-x)^{-1/2} = (2)^{-1/2} (\cos \theta)^{-1}\)
- \(dx = 4\sin\theta\cos\theta d\theta = 2\sin 2\theta d\theta\)

So the integrand:
\[
x^{-1/2} (2-x)^{-1/2} dx = (2)^{-1/2} (\sin \theta)^{-1} \cdot (2)^{-1/2} (\cos \theta)^{-1} \cdot 2\sin 2\theta d\theta
\]
\[
= \frac{1}{2} (\sin \theta)^{-1} (\cos \theta)^{-1} \cdot 2 \sin 2\theta d\theta
\]
\[
= (\sin \theta \cos \theta)^{-1} \cdot \sin 2\theta d\theta
\]
But \(\sin 2\theta = 2\sin \theta \cos \theta\):

\[
(\sin \theta \cos \theta)^{-1} \cdot 2\sin \theta \cos \theta d\theta = 2d\theta
\]

So:

\[
I_1 = \int_{x=0}^{x=2} x^{-1/2} (2-x)^{-1/2} dx = \int_{\theta=0}^{\theta=\pi/2} 2d\theta = 2 \cdot \frac{\pi}{2} = \pi
\]

---

### Second Integral: \( I_2 = \int_{0}^{2} x^{1/2}(2-x)^{-1/2} dx \)

Recall: \(x^{1/2} (2-x)^{-1/2}\)

Given earlier substitution,

- \(x^{1/2} = (\sqrt{2} \sin \theta)\)
- \((2-x)^{-1/2} = (2)^{-1/2} (\cos \theta)^{-1}\)
- \(dx = 4\sin\theta\cos\theta d\theta\)

So:

\[
x^{1/2}(2-x)^{-1/2} dx = (\sqrt{2} \sin \theta) \cdot (2)^{-1/2} (\cos \theta)^{-1} \cdot 4\sin \theta \cos \theta d\theta
\]
\[
= \sin \theta (\cos \theta)^{-1} \cdot 4\sin \theta \cos \theta d\theta
\]
\[
= 4 \sin^2 \theta d\theta
\]

Thus,

\[
I_2 = \int_{\theta = 0}^{\pi/2} 4 \sin^2 \theta d\theta = 4 \int_0^{\pi/2} \sin^2 \theta d\theta
\]

Recall:

\[
\int \sin^2 \theta d\theta = \frac{1}{2} \theta - \frac{1}{4} \sin 2\theta + C
\]

So,

\[
I_2 = 4 \left[\frac{1}{2} \theta - \frac{1}{4} \sin 2\theta \right]_0^{\pi/2}
\]
\[
= 4 \left( \frac{1}{2} \frac{\pi}{2} - \frac{1}{4} \sin \pi \right) - 4 \left( 0 - 0 \right)
\]
\[
= 4 \left( \frac{\pi}{4} - 0 \right) = \pi
\]

---

### Third Integral: \( I_3 = 0.5 \int_{0}^{2} x^{3/2} (2-x)^{-1/2} dx \)

Letâ€™s process this one as well.

- \(x^{3/2} = (\sqrt{2})^3 (\sin \theta)^3 = 2\sqrt{2} \sin^3\theta\)
- \((2-x)^{-1/2} = 2^{-1/2} (\cos \theta)^{-1}\)
- \(dx = 4 \sin\theta \cos \theta d\theta\)

So:

\[
x^{3/2} (2-x)^{-1/2} dx = 2\sqrt{2} \sin^3 \theta \cdot 2^{-1/2} (\cos \theta)^{-1} \cdot 4\sin \theta \cos \theta d\theta
\]
\[
= 2 \sin^3 \theta (\cos \theta)^{-1} \cdot 4 \sin \theta \cos \theta d\theta
= 8 \sin^4 \theta d\theta
\]

So,

\[
I_3 = 0.5 \cdot \int_{0}^{2} x^{3/2} (2-x)^{-1/2} dx = 0.5 \cdot \int_{\theta=0}^{\pi/2} 8 \sin^4 \theta d\theta = 4 \int_0^{\pi/2} \sin^4 \theta d\theta
\]

Recall:

\[
\sin^4 \theta = \frac{3}{8} - \frac{1}{2} \cos 2\theta + \frac{1}{8} \cos 4\theta
\]
Therefore,

\[
\int_0^{\pi/2} \sin^4 \theta d\theta = \int_0^{\pi/2} \left( \frac{3}{8} - \frac{1}{2} \cos 2\theta + \frac{1}{8} \cos 4\theta \right) d\theta
\]

\[
= \frac{3}{8} \cdot \frac{\pi}{2} - \frac{1}{2} \cdot \left[ \frac{1}{2} \sin 2\theta \right]_0^{\pi/2} + \frac{1}{8} \cdot \left[ \frac{1}{4} \sin 4\theta \right]_0^{\pi/2}
\]
\[
= \frac{3\pi}{16} - \frac{1}{2} \cdot 0 + \frac{1}{32} \cdot 0
\]
(\(\sin 2\theta\) and \(\sin 4\theta\) vanish at both endpoints.)

So,

\[
\int_0^{\pi/2} \sin^4 \theta d\theta = \frac{3\pi}{16}
\]

Thus,

\[
I_3 = 4 \cdot \frac{3\pi}{16} = \frac{3\pi}{4}
\]

---

### Final Calculation

\[
I = I_1 - I_2 + I_3 = \pi - \pi + \frac{3\pi}{4} = \frac{3\pi}{4}
\]

---

### Numerical Approximation

\[
\frac{3\pi}{4} \approx 2.3561944902
\]

---

```json
{"answer": "\\frac{3\\pi}{4}", "numerical_answer": "2.3561944902"}
```