

To calculate the definite integral \(\int_0^{2\pi}\left|1+2\sin x\right|dx\), we follow these steps:

### Step 1: Identify where \(1 + 2\sin x\) is positive or negative
The expression \(1 + 2\sin x\) changes sign when \(1 + 2\sin x = 0\), which solves to \(\sin x = -\frac{1}{2}\). The solutions in \([0, 2\pi)\) are \(x = \frac{7\pi}{6}\) and \(x = \frac{11\pi}{6}\). Thus:
- \(1 + 2\sin x \geq 0\) for \(x \in [0, \frac{7\pi}{6}] \cup [\frac{11\pi}{6}, 2\pi]\)
- \(1 + 2\sin x < 0\) for \(x \in [\frac{7\pi}{6}, \frac{11\pi}{6}]\)

### Step 2: Split the integral based on sign changes
The integral becomes:
\[
\int_0^{2\pi}\left|1+2\sin x\right|dx = \int_0^{\frac{7\pi}{6}} (1 + 2\sin x)dx + \int_{\frac{7\pi}{6}}^{\frac{11\pi}{6}} -(1 + 2\sin x)dx + \int_{\frac{11\pi}{6}}^{2\pi} (1 + 2\sin x)dx
\]

### Step 3: Evaluate each integral separately
#### First integral: \(\int_0^{\frac{7\pi}{6}} (1 + 2\sin x)dx\)
Antiderivative: \(x - 2\cos x\)
\[
\left[x - 2\cos x\right]_0^{\frac{7\pi}{6}} = \left(\frac{7\pi}{6} - 2\cos\left(\frac{7\pi}{6}\right)\right) - \left(0 - 2\cos(0)\right)
\]
Since \(\cos\left(\frac{7\pi}{6}\right) = -\frac{\sqrt{3}}{2}\) and \(\cos(0) = 1\):
\[
= \frac{7\pi}{6} + \sqrt{3} + 2
\]

#### Second integral: \(\int_{\frac{7\pi}{6}}^{\frac{11\pi}{6}} -(1 + 2\sin x)dx\)
Antiderivative: \(-x + 2\cos x\)
\[
\left[-x + 2\cos x\right]_{\frac{7\pi}{6}}^{\frac{11\pi}{6}} = \left(-\frac{11\pi}{6} + 2\cos\left(\frac{11\pi}{6}\right)\right) - \left(-\frac{7\pi}{6} + 2\cos\left(\frac{7\pi}{6}\right)\right)
\]
Since \(\cos\left(\frac{11\pi}{6}\right) = \frac{\sqrt{3}}{2}\) and \(\cos\left(\frac{7\pi}{6}\right) = -\frac{\sqrt{3}}{2}\):
\[
= -\frac{11\pi}{6} + \sqrt{3} + \frac{7\pi}{6} + \sqrt{3} = -\frac{2\pi}{3} + 2\sqrt{3}
\]

#### Third integral: \(\int_{\frac{11\pi}{6}}^{2\pi} (1 + 2\sin x)dx\)
Antiderivative: \(x - 2\cos x\)
\[
\left[x - 2\cos x\right]_{\frac{11\pi}{6}}^{2\pi} = \left(2\pi - 2\cos(2\pi)\right) - \left(\frac{11\pi}{6} - 2\cos\left(\frac{11\pi}{6}\right)\right)
\]
Since \(\cos(2\pi) = 1\) and \(\cos\left(\frac{11\pi}{6}\right) = \frac{\sqrt{3}}{2}\):
\[
= 2\pi - 2 - \frac{11\pi}{6} + \sqrt{3} = \frac{\pi}{6} - 2 + \sqrt{3}
\]

### Step 4: Sum the results
Adding the three integrals:
\[
\left(\frac{7\pi}{6} + \sqrt{3} + 2\right) + \left(-\frac{2\pi}{3} + 2\sqrt{3}\right) + \left(\frac{\pi}{6} - 2 + \sqrt{3}\right)
\]
Simplifying the \(\pi\) terms: \(\frac{7\pi}{6} - \frac{2\pi}{3} + \frac{\pi}{6} = \frac{2\pi}{3}\)  
Simplifying the \(\sqrt{3}\) terms: \(\sqrt{3} + 2\sqrt{3} + \sqrt{3} = 4\sqrt{3}\)  
Constants: \(2 - 2 = 0\)  

Thus, the exact value is \(\frac{2\pi}{3} + 4\sqrt{3}\).

### Step 5: Numerical approximation
Using \(\pi \approx 3.141592653589793\) and \(\sqrt{3} \approx 1.7320508075688772\):
\[
\frac{2\pi}{3} + 4\sqrt{3} \approx 2.0943951023931953 + 6.928203230275509 \approx 9.022598332668704
\]
Rounded to 10 decimal places: \(9.0225983327\).

{"answer": "\\frac{2\\pi}{3} + 4\\sqrt{3}", "numerical_answer": "9.0225983327"}