# Evaluating $\int_{-1}^1 x^2 \cdot \sqrt[3]{x^3+1} \, dx$

## Step 1: Make a substitution

Let's use the substitution $u = x^3 + 1$, then:
- $du = 3x^2 \, dx$
- $x^2 \, dx = \frac{du}{3}$

When $x = -1$, $u = (-1)^3 + 1 = -1 + 1 = 0$
When $x = 1$, $u = 1^3 + 1 = 1 + 1 = 2$

## Step 2: Rewrite the integral in terms of $u$

$\int_{-1}^1 x^2 \cdot \sqrt[3]{x^3+1} \, dx = \int_{-1}^1 x^2 \cdot (x^3+1)^{1/3} \, dx = \int_{0}^2 \frac{1}{3} \cdot u^{1/3} \, du$

$= \frac{1}{3} \int_{0}^2 u^{1/3} \, du$

## Step 3: Evaluate the integral

$\frac{1}{3} \int_{0}^2 u^{1/3} \, du = \frac{1}{3} \cdot \frac{u^{4/3}}{\frac{4}{3}} \Bigg|_{0}^{2} = \frac{1}{3} \cdot \frac{3}{4} \cdot u^{4/3} \Bigg|_{0}^{2}$

$= \frac{1}{4} \cdot u^{4/3} \Bigg|_{0}^{2} = \frac{1}{4} \cdot (2^{4/3} - 0^{4/3})$

$= \frac{1}{4} \cdot 2^{4/3} = \frac{2^{4/3}}{4}$

## Step 4: Simplify the result

$\frac{2^{4/3}}{4} = \frac{2^{4/3}}{2^2} = 2^{4/3-2} = 2^{1/3} \cdot 2^{-1} = \frac{2^{1/3}}{2} = \frac{\sqrt[3]{2}}{2}$

## Step 5: Numerical approximation

The numerical value of $\frac{\sqrt[3]{2}}{2}$ is approximately $0.6299605249$ (rounded to 10 decimal places).

To verify: $\sqrt[3]{2} \approx 1.2599210498$ and dividing by 2 gives $\frac{1.2599210498}{2} \approx 0.6299605249$

{"answer": "\\frac{\\sqrt[3]{2}}{2}", "numerical_answer": "0.6299605249"}