To evaluate the definite integral

$$
\int_0^\infty \frac{x^3}{e^x - 1} \left[8\cosh\left(\frac{x}{2}\right) - \cosh\left(\frac{x}{4}\right)\right] dx,
$$

we proceed by expanding the hyperbolic cosine terms and the denominator using known series representations.

---

### Step 1: Expand the integrand

Recall the identity:

$$
\frac{1}{e^x - 1} = \sum_{n=1}^\infty e^{-nx}.
$$

Also, using the exponential definition of hyperbolic cosine:

$$
\cosh(ax) = \frac{e^{ax} + e^{-ax}}{2},
$$

we expand the bracketed expression:

$$
8\cosh\left(\frac{x}{2}\right) - \cosh\left(\frac{x}{4}\right)
= 4\left(e^{x/2} + e^{-x/2}\right) - \frac{1}{2}\left(e^{x/4} + e^{-x/4}\right).
$$

Substituting into the integral:

$$
\int_0^\infty x^3 \left(\sum_{n=1}^\infty e^{-nx}\right) \left[4\left(e^{x/2} + e^{-x/2}\right) - \frac{1}{2}\left(e^{x/4} + e^{-x/4}\right)\right] dx.
$$

Now distribute the sum and the exponential terms:

$$
\sum_{n=1}^\infty \left[4\int_0^\infty x^3 e^{-(n - 1/2)x} dx + 4\int_0^\infty x^3 e^{-(n + 1/2)x} dx - \frac{1}{2}\int_0^\infty x^3 e^{-(n - 1/4)x} dx - \frac{1}{2}\int_0^\infty x^3 e^{-(n + 1/4)x} dx\right].
$$

---

### Step 2: Evaluate each integral

Using the standard result:

$$
\int_0^\infty x^3 e^{-kx} dx = \frac{6}{k^4},
$$

we substitute into the sum:

$$
\sum_{n=1}^\infty \left[\frac{24}{(n - 1/2)^4} + \frac{24}{(n + 1/2)^4} - \frac{3}{(n - 1/4)^4} - \frac{3}{(n + 1/4)^4} \right].
$$

This can be written compactly as:

$$
\sum_{n=1}^\infty \left[24\left(\frac{1}{(n - 1/2)^4} + \frac{1}{(n + 1/2)^4}\right) - 3\left(\frac{1}{(n - 1/4)^4} + \frac{1}{(n + 1/4)^4}\right)\right].
$$

---

### Step 3: Express in terms of Hurwitz zeta functions

We now recognize that these sums are related to the Hurwitz zeta function:

$$
\zeta(s, a) = \sum_{n=0}^\infty \frac{1}{(n + a)^s}.
$$

Using this, we rewrite the sums:

- $ \sum_{n=1}^\infty \frac{1}{(n - 1/2)^4} = \sum_{m=0}^\infty \frac{1}{(m + 1/2)^4} = \zeta(4, 1/2) $
- $ \sum_{n=1}^\infty \frac{1}{(n + 1/2)^4} = \zeta(4, 3/2) $
- $ \sum_{n=1}^\infty \frac{1}{(n - 1/4)^4} = \zeta(4, 3/4) $
- $ \sum_{n=1}^\infty \frac{1}{(n + 1/4)^4} = \zeta(4, 5/4) $

So the total becomes:

$$
24\left[\zeta(4, 1/2) + \zeta(