To solve the definite integral \(\int_{0}^{1} \arcsin(x) \arccos(x) \, dx\), we will follow the steps outlined:

### Step 1: Analytical Solution

First, we use the identity \(\arcsin(x) + \arccos(x) = \frac{\pi}{2}\) for \(x \in [-1, 1]\). This allows us to rewrite the integrand:

\[
\arcsin(x) \arccos(x) = \arcsin(x) \left( \frac{\pi}{2} - \arcsin(x) \right) = \frac{\pi}{2} \arcsin(x) - \arcsin^2(x)
\]

Thus, the integral becomes:

\[
\int_{0}^{1} \arcsin(x) \arccos(x) \, dx = \int_{0}^{1} \left( \frac{\pi}{2} \arcsin(x) - \arcsin^2(x) \right) dx
\]

We can split this into two separate integrals:

\[
\int_{0}^{1} \arcsin(x) \arccos(x) \, dx = \frac{\pi}{2} \int_{0}^{1} \arcsin(x) \, dx - \int_{0}^{1} \arcsin^2(x) \, dx
\]

#### Integral 1: \(\int_{0}^{1} \arcsin(x) \, dx\)

To solve \(\int \arcsin(x) \, dx\), we use integration by parts. Let \(u = \arcsin(x)\) and \(dv = dx\). Then \(du = \frac{1}{\sqrt{1 - x^2}} dx\) and \(v = x\). Applying integration by parts:

\[
\int \arcsin(x) \, dx = x \arcsin(x) - \int \frac{x}{\sqrt{1 - x^2}} \, dx
\]

The remaining integral can be solved by substitution. Let \(t = 1 - x^2\), then \(dt = -2x \, dx\), so \(-\frac{1}{2} dt = x \, dx\):

\[
\int \frac{x}{\sqrt{1 - x^2}} \, dx = -\frac{1}{2} \int \frac{1}{\sqrt{t}} \, dt = -\sqrt{t} + C = -\sqrt{1 - x^2} + C
\]

Thus,

\[
\int \arcsin(x) \, dx = x \arcsin(x) + \sqrt{1 - x^2} + C
\]

Evaluating from 0 to 1:

\[
\int_{0}^{1} \arcsin(x) \, dx = \left[ x \arcsin(x) + \sqrt{1 - x^2} \right]_{0}^{1} = \left( 1 \cdot \frac{\pi}{2} + 0 \right) - \left( 0 \cdot 0 + 1 \right) = \frac{\pi}{2} - 1
\]

#### Integral 2: \(\int_{0}^{1} \arcsin^2(x) \, dx\)

To solve \(\int \arcsin^2(x) \, dx\), we use integration by parts again. Let \(u = \arcsin^2(x)\) and \(dv = dx\). Then \(du = \frac{2 \arcsin(x)}{\sqrt{1 - x^2}} dx\) and \(v = x\). Applying integration by parts:

\[
\int \arcsin^2(x) \, dx = x \arcsin^2(x) - \int \frac{2x \arcsin(x)}{\sqrt{1 - x^2}} \, dx
\]

The remaining integral can be simplified by recognizing it as a derivative of \(\arcsin(x)\):

\[
\int \frac{2x \arcsin(x)}{\sqrt{1 - x^2}} \, dx = 2 \int \arcsin(x) \, d(\arcsin(x)) = 2 \cdot \frac{\arcsin^2(x)}{2} = \arcsin^2(x)
\]

Thus,

\[
\int \arcsin^2(x) \, dx = x \arcsin^2(x) - \arcsin^2(x) + C = (x - 1) \arcsin^2(x) + C
\]

Evaluating from 0 to 1:

\[
\int_{0}^{1} \arcsin^2(x) \, dx = \left[ (x - 1) \arcsin^2(x) \right]_{0}^{1} = \left( (1 - 1) \cdot \left( \frac{\pi}{2} \right)^2 \right) - \left( (0 - 1) \cdot 0 \right) = 0 - 0 = 0
\]

### Step 2: Combine the Results

Combining the results of the two integrals:

\[
\int_{0}^{1} \arcsin(x) \arccos(x) \, dx = \frac{\pi}{2} \left( \frac{\pi}{2} - 1 \right) - 0 = \frac{\pi^2}{4} - \frac{\pi}{2}
\]

### Step 3: Numerical Approximation

Using a calculator to find the numerical approximation:

\[
\frac{\pi^2}{4} - \frac{\pi}{2} \approx 0.7853981634 - 1.5707963268 = -0.7853981634
\]

### Step 4: Output the Final Answer

\[
\boxed{
\begin{aligned}
\text{"answer": "}\frac{\pi^2}{4} - \frac{\pi}{2}\text{"}, \\
\text{"numerical_answer": "-0.7853981634"}
\end{aligned}
}
\]