

To solve the definite integral \(\int_{0}^{2} x^{-1/2}(2 - x)^{-1/2} \cos\left(\sqrt{x(2 - x)}\right) \, dx\), we proceed with the following steps:

### Step 1: Substitution to Simplify the Integrand
Let \( x = 2 \sin^2 \theta \). This substitution transforms the limits of integration: when \( x = 0 \), \( \theta = 0 \); when \( x = 2 \), \( \theta = \pi/2 \). 

First, compute \( 2 - x \):
\[
2 - x = 2 - 2 \sin^2 \theta = 2 \cos^2 \theta.
\]
Next, the product \( x(2 - x) \) becomes:
\[
x(2 - x) = (2 \sin^2 \theta)(2 \cos^2 \theta) = 4 \sin^2 \theta \cos^2 \theta = (2 \sin \theta \cos \theta)^2 = \sin^2(2\theta).
\]
Thus, \( \sqrt{x(2 - x)} = \sin(2\theta) \).

The differential \( dx \) is:
\[
dx = \frac{d}{d\theta} \left(2 \sin^2 \theta\right) d\theta = 4 \sin \theta \cos \theta \, d\theta.
\]

### Step 2: Rewrite the Integral in Terms of \(\theta\)
The integrand \( x^{-1/2}(2 - x)^{-1/2} \cos\left(\sqrt{x(2 - x)}\right) \) becomes:
\[
\left[ (2 \sin^2 \theta)(2 \cos^2 \theta) \right]^{-1/2} \cos(\sin(2\theta)) \cdot 4 \sin \theta \cos \theta \, d\theta.
\]
Simplify the first term:
\[
\left[4 \sin^2 \theta \cos^2 \theta\right]^{-1/2} = \frac{1}{2 \sin \theta \cos \theta}.
\]
Thus, the integrand simplifies to:
\[
\frac{1}{2 \sin \theta \cos \theta} \cdot \cos(\sin(2\theta)) \cdot 4 \sin \theta \cos \theta \, d\theta = 2 \cos(\sin(2\theta)) \, d\theta.
\]
The integral now becomes:
\[
\int_{0}^{\pi/2} 2 \cos(\sin(2\theta)) \, d\theta.
\]

### Step 3: Further Substitution to Simplify the Integral
Let \( \phi = 2\theta \), so \( d\phi = 2 \, d\theta \) (i.e., \( d\theta = d\phi/2 \)). The limits of integration change from \( \theta = 0 \) to \( \theta = \pi/2 \) to \( \phi = 0 \) to \( \phi = \pi \). The integral becomes:
\[
\int_{0}^{\pi} \cos(\sin \phi) \, d\phi.
\]

### Step 4: Recognize the Integral as a Bessel Function
The integral \( \int_{0}^{\pi} \cos(\sin \phi) \, d\phi \) is a standard form related to the Bessel function of the first kind, \( J_0(z) \). The integral representation of \( J_0(z) \) is:
\[
J_0(z) = \frac{1}{\pi} \int_{0}^{\pi} \cos(z \sin \phi) \, d\phi.
\]
For \( z = 1 \), this gives:
\[
\int_{0}^{\pi} \cos(\sin \phi) \, d\phi = \pi J_0(1).
\]

### Step 5: Final Result
Thus, the original integral simplifies to \( \pi J_0(1) \).

### Numerical Approximation
The Bessel function \( J_0(1) \approx 0.7651976865579666 \). Multiplying by \( \pi \approx 3.141592653589793 \), we get:
\[
\pi J_0(1) \approx 2.403923288.
\]

{"answer": "\(\pi J_0(1)\)", "numerical_answer": "2.4039232880"}