# Evaluating $\int\limits_{0}^{2}x^{-1/2}(2-x)^{-1/2}\cosh\left(1\sqrt{x(2-x)}\right)dx$

## Step 1: Recognize the structure of the integral

First, I'll examine the integrand $x^{-1/2}(2-x)^{-1/2}\cosh\left(1\sqrt{x(2-x)}\right)$

Looking at the form, I notice we have:
- $x^{-1/2}(2-x)^{-1/2}$ term
- $\cosh\left(1\sqrt{x(2-x)}\right)$ term

Let's consider a substitution to simplify this integral.

## Step 2: Apply a substitution

The expression $x(2-x)$ suggests we might use a trigonometric substitution.

Let's try $x = 1 - \cos(\theta)$ or equivalently $x = 1 + \cos(\phi)$ where $\phi = \theta - \pi$

With $x = 1 + \cos(\phi)$, we get:
- $2-x = 2-(1+\cos(\phi)) = 1-\cos(\phi)$
- $x(2-x) = (1+\cos(\phi))(1-\cos(\phi)) = 1-\cos^2(\phi) = \sin^2(\phi)$
- $dx = -\sin(\phi)d\phi$

When $x = 0$, we have $1+\cos(\phi) = 0$, so $\cos(\phi) = -1$ and $\phi = \pi$
When $x = 2$, we have $1+\cos(\phi) = 2$, so $\cos(\phi) = 1$ and $\phi = 0$

## Step 3: Transform the integral

Now, we can rewrite the integral:

$x^{-1/2} = (1+\cos(\phi))^{-1/2}$
$(2-x)^{-1/2} = (1-\cos(\phi))^{-1/2}$
$\cosh(1\sqrt{x(2-x)}) = \cosh(\sin(\phi))$
$dx = -\sin(\phi)d\phi$

So our integral becomes:
$\int_{\pi}^{0} (1+\cos(\phi))^{-1/2}(1-\cos(\phi))^{-1/2}\cosh(\sin(\phi))(-\sin(\phi))d\phi$

Simplifying:
$\int_{0}^{\pi} (1+\cos(\phi))^{-1/2}(1-\cos(\phi))^{-1/2}\cosh(\sin(\phi))\sin(\phi)d\phi$

## Step 4: Simplify the integrand

We know that:
$(1+\cos(\phi))^{-1/2}(1-\cos(\phi))^{-1/2} = \frac{1}{\sqrt{(1+\cos(\phi))(1-\cos(\phi))}} = \frac{1}{\sqrt{\sin^2(\phi)}} = \frac{1}{|\sin(\phi)|} = \frac{1}{\sin(\phi)}$ (since $\sin(\phi) > 0$ in $(0,\pi)$)

So our integral becomes:
$\int_{0}^{\pi} \frac{\cosh(\sin(\phi))\sin(\phi)}{\sin(\phi)}d\phi = \int_{0}^{\pi} \cosh(\sin(\phi))d\phi$

## Step 5: Use symmetry property

Since $\sin(\pi-\phi) = \sin(\phi)$ and $\cosh$ is an even function, $\cosh(\sin(\pi-\phi)) = \cosh(\sin(\phi))$

This means our integrand is symmetric around $\phi = \pi/2$, so:
$\int_{0}^{\pi} \cosh(\sin(\phi))d\phi = 2\int_{0}^{\pi/2} \cosh(\sin(\phi))d\phi$

## Step 6: Evaluate the integral

For an integral of the form $\int \cosh(\sin(\phi))d\phi$, we can use the fact that:
$\int \cosh(\sin(\phi))d\phi = \pi I_0(1)$, where $I_0$ is the modified Bessel function of the first kind of order 0.

Therefore:
$2\int_{0}^{\pi/2} \cosh(\sin(\phi))d\phi = 2 \cdot \frac{\pi}{2} I_0(1) = \pi I_0(1)$

## Step 7: Final result

The exact value of our integral is:
$\int\limits_{0}^{2}x^{-1/2}(2-x)^{-1/2}\cosh\left(1\sqrt{x(2-x)}\right)dx = \pi I_0(1)$

The numerical value of $I_0(1)$ is approximately 1.2660658777, so:
$\pi I_0(1) \approx \pi \cdot 1.2660658777 \approx 3.9771463315$

## Final answer

{"answer": "\pi I_0(1)", "numerical_answer": "3.9771463315"}