# Calculating $\int_{0}^{1}{\frac{x^{3}+x+1}{3x^{2}-3x+4}}\:\mathrm{d}x$

## Step 1: Divide the numerator by the denominator

I'll perform polynomial long division to express the integrand in a more manageable form.

$$\frac{x^3+x+1}{3x^2-3x+4}$$

First, let's divide $x^3$ by $3x^2$:
- $\frac{x^3}{3x^2} = \frac{x}{3}$
- Multiply: $\frac{x}{3} \cdot (3x^2-3x+4) = x^3-x^2+\frac{4x}{3}$
- Subtract: $x^3+x+1 - (x^3-x^2+\frac{4x}{3}) = x^2+x-\frac{4x}{3}+1 = x^2+\frac{3x-4x}{3}+1 = x^2-\frac{x}{3}+1$

Continuing:
- $\frac{x^2}{3x^2} = \frac{1}{3}$
- Multiply: $\frac{1}{3} \cdot (3x^2-3x+4) = x^2-x+\frac{4}{3}$
- Subtract: $x^2-\frac{x}{3}+1 - (x^2-x+\frac{4}{3}) = -\frac{x}{3}+x+1-\frac{4}{3} = \frac{2x}{3}-\frac{1}{3}$

Therefore:
$$\frac{x^3+x+1}{3x^2-3x+4} = \frac{x}{3} + \frac{1}{3} + \frac{\frac{2x}{3}-\frac{1}{3}}{3x^2-3x+4}$$

## Step 2: Simplify the remainder term

Let's work with the remainder term:
$$\frac{\frac{2x}{3}-\frac{1}{3}}{3x^2-3x+4} = \frac{2x-1}{3(3x^2-3x+4)}$$

We need to complete the square in the denominator:
$$3x^2-3x+4 = 3(x^2-x) + 4 = 3(x^2-x+\frac{1}{4}) + 4 - \frac{3}{4} = 3(x-\frac{1}{2})^2 + \frac{13}{4}$$

So our remainder term becomes:
$$\frac{2x-1}{3(3(x-\frac{1}{2})^2 + \frac{13}{4})} = \frac{2x-1}{9(x-\frac{1}{2})^2 + \frac{39}{4}}$$

Let's substitute $u = x-\frac{1}{2}$ to simplify further:
When $x = u + \frac{1}{2}$, we get:
$$\frac{2(u+\frac{1}{2})-1}{9u^2 + \frac{39}{4}} = \frac{2u+1-1}{9u^2 + \frac{39}{4}} = \frac{2u}{9u^2 + \frac{39}{4}}$$

This can be rewritten as:
$$\frac{2u}{9u^2 + \frac{39}{4}} = \frac{8u}{36u^2 + 39}$$

## Step 3: Integrate each term

Our integral is now:
$$\int_{0}^{1}\left(\frac{x}{3} + \frac{1}{3} + \frac{8(x-\frac{1}{2})}{36(x-\frac{1}{2})^2 + 39}\right)\,dx$$

The first two terms are straightforward:
$$\int\frac{x}{3}\,dx = \frac{x^2}{6} + C_1$$
$$\int\frac{1}{3}\,dx = \frac{x}{3} + C_2$$

For the third term, let's substitute $u = x-\frac{1}{2}$, which gives $dx = du$ and changes the bounds:
- When $x = 0$, $u = -\frac{1}{2}$
- When $x = 1$, $u = \frac{1}{2}$

So we have:
$$\int_{-\frac{1}{2}}^{\frac{1}{2}}\frac{8u}{36u^2 + 39}\,du$$

Using the substitution $v = 6u$, we get $du = \frac{dv}{6}$ and:
$$\int_{-3}^{3}\frac{8\frac{v}{6}}{36\frac{v^2}{36} + 39}\cdot\frac{dv}{6} = \frac{8}{36}\int_{-3}^{3}\frac{v}{v^2 + 39}\,dv$$

This can be integrated using the formula $\int\frac{v}{v^2+a^2}\,dv = \frac{1}{2}\ln(v^2+a^2) + C$:
$$\frac{8}{36}\int_{-3}^{3}\frac{v}{v^2 + 39}\,dv = \frac{8}{36}\cdot\frac{1}{2}\ln(v^2+39)\big|_{-3}^{3} = \frac{4}{36}\ln(v^2+39)\big|_{-3}^{3}$$

Since $v^2+39$ is the same for $v = 3$ and $v = -3$, this evaluates to 0.

## Step 4: Evaluate the definite integral

Now we evaluate the other terms at the bounds:
$$\left[\frac{x^2}{6} + \frac{x}{3}\right]_{0}^{1} = \left(\frac{1}{6} + \frac{1}{3}\right) - \left(0 + 0\right) = \frac{1}{6} + \frac{1}{3} = \frac{1}{6} + \frac{2}{6} = \frac{3}{6} = \frac{1}{2}$$

## Step 5: Calculate the numerical approximation

The exact answer is $\frac{1}{2}$, which as a decimal is 0.5000000000 (to 10 decimal places).

Therefore, the value of the definite integral $\int_{0}^{1}{\frac{x^{3}+x+1}{3x^{2}-3x+4}}\:\mathrm{d}x = \frac{1}{2}$.

{"answer": "\\frac{1}{2}", "numerical_answer": "0.5000000000"}