

To solve the definite integral \(\int_0^{2\pi}\sin(\sin(x)-x)\, dx\), we proceed as follows:

### Step 1: Analytic Evaluation
Let \( I = \int_0^{2\pi}\sin(\sin(x) - x)\, dx \). We use the substitution \( u = 2\pi - x \), which transforms the integral. When \( x = 0 \), \( u = 2\pi \); when \( x = 2\pi \), \( u = 0 \). The differential \( dx = -du \), so the integral becomes:
\[
I = \int_{2\pi}^0 \sin\left(\sin(2\pi - u) - (2\pi - u)\right) (-du) = \int_0^{2\pi} \sin\left(\sin(2\pi - u) - 2\pi + u\right) du.
\]
Since \(\sin(2\pi - u) = -\sin(u)\), the argument of the sine function simplifies to:
\[
\sin(2\pi - u) - 2\pi + u = -\sin(u) - 2\pi + u = (u - \sin(u)) - 2\pi.
\]
Using the periodicity of the sine function (\(\sin(\theta - 2\pi) = \sin(\theta)\)), we have:
\[
\sin\left((u - \sin(u)) - 2\pi\right) = \sin(u - \sin(u)).
\]
Thus, the integral becomes:
\[
I = \int_0^{2\pi} \sin(u - \sin(u))\, du.
\]
However, the original integrand is \(\sin(\sin(x) - x) = \sin(-(x - \sin(x))) = -\sin(x - \sin(x))\). Therefore:
\[
I = \int_0^{2\pi} -\sin(x - \sin(x))\, dx = -\int_0^{2\pi} \sin(x - \sin(x))\, dx.
\]
Comparing the two expressions for \( I \), we find \( I = -I \), which implies \( 2I = 0 \), so \( I = 0 \).

### Step 2: Numerical Approximation
Since the exact value of the integral is \( 0 \), the numerical approximation (rounded to 10 decimal places) is \( 0.0000000000 \).

{"answer": "0", "numerical_answer": "0.0000000000"}