We wish to evaluate

  I = ∫₀¹ [sin(log x) – log x]⁄[log²x] dx.

Step 1. Change of Variables

Let u = log x, so that x = eᵘ and dx = eᵘ du. When x = 0, u → –∞, and when x = 1, u = 0. Then

  I = ∫₋∞⁰ [sin u – u]⁄[u²] · eᵘ du.

It is often useful to reverse the sign by substituting t = –u. Then u = –t and du = –dt. When u goes from –∞ to 0, t goes from ∞ to 0. Changing the limits and simplifying we have

  I = ∫₀∞ [ ( (–t) sin? – (–t)? ] 
       
Let’s do it step by step. Under the substitution, we have

  sin u = sin(–t) = – sin t,
  log stuff: u = –t, so u² = t²,
  eᵘ = e^(–t).

Thus,
  I = ∫₋∞⁰ [sin u – u]⁄[u²] eᵘ du
    = ∫∞⁰ [sin(–t) – (–t)]⁄[t²] e^(–t) (–dt)
    = ∫₀∞ [– sin t + t]⁄[t²] e^(–t) dt
    = ∫₀∞ [t – sin t] e^(–t)/t² dt.

Step 2. An Integral Representation

We now need to evaluate

  I = ∫₀∞ (t – sin t) e^(–t)/t² dt.

A useful observation is that

  1 – sin t/t = ∫₀¹ [1 – cos(ut)] du,
 
because
  ∫₀¹ cos(ut) du = (sin t)/(t).

Thus, multiplying by t we have

  t – sin t = t(1 – sin t/t) = t∫₀¹ [1 – cos(ut)] du.

Substitute this in I:

  I = ∫₀∞ [t∫₀¹ (1 – cos(ut)) du] e^(–t)/t² dt
    = ∫₀¹ [∫₀∞ (1 – cos(ut)) e^(–t)/t dt] du.

Step 3. Changing the Order of Integration and Evaluating the Inner Integral

Define
  J(u) = ∫₀∞ (1 – cos(ut)) e^(–t)/t dt.

To evaluate J(u), think of u as a parameter. Differentiate with respect to u:

  dJ/du = ∫₀∞ (d/du)[1 – cos(ut)] e^(–t)/t dt
      = ∫₀∞ sin(ut)·t e^(–t)/t dt = ∫₀∞ sin(ut) e^(–t) dt.

The Laplace transform of sin(ut) is
  ∫₀∞ sin(ut) e^(–t) dt = u/(1 + u²).
Thus,
  dJ/du = u/(1 + u²).

Since J(0) = 0 (because cos 0 = 1), we integrate:

  J(u) = ∫₀ᵘ [s/(1+s²)] ds = ½ ln(1+s²) |₀ᵘ = ½ ln(1+u²).

Now our integral becomes

  I = ∫₀¹ J(u) du = ½ ∫₀¹ ln(1+u²) du.

Step 4. Evaluating ∫₀¹ ln(1+u²) du

We use integration by parts. Let

  v = ln(1+u²)  ⇒  dv = (2u/(1+u²)) du,
  dw = du      ⇒  w = u.

Then,
  ∫ ln(1+u²) du = u ln(1+u²) – ∫ u (2u/(1+u²)) du
        = u ln(1+u²) – 2∫ (u²/(1+u²)) du.
Notice that
  u²/(1+u²) = 1 – 1/(1+u²),
so
  ∫ ln(1+u²) du = u ln(1+u²) – 2∫ (1 – 1/(1+u²)) du
        = u ln(1+u²) – 2[u – arctan u] + C.
Thus, evaluating from 0 to 1,

  ∫₀¹ ln(1+u²) du = [1·ln2 – 2(1 – arctan 1)] – [0 – 0]
        = ln 2 – 2(1 – π/4)
        = ln 2 – 2 + (π/2).

Step 5. Final Answer

Thus, recalling that

  I = ½ · (ln 2 – 2 + (π/2)) = (π/4) + (½ ln 2) – 1.

Step 6. Numerical Approximation

We now approximate:
  π/4 ≈ 0.7853981634,
  ½ ln 2 ≈ 0.3465735904 (since ln 2 ≈ 0.6931471806),
  so I ≈ 0.7853981634 + 0.3465735904 − 1 = 0.1319717538.

Thus, the final answers are:

Exact answer: (π/4) + (½ ln 2) − 1
Numerical answer: 0.1319717538

{"answer": "\\frac{\\pi}{4} + \\frac{1}{2}\\ln 2 - 1", "numerical_answer": "0.1319717538"}