Let's solve the definite integral step by step:

\[
I = \int_{0}^{2}\frac{x^{-1/2}(2-x)^{-1/2}}{\sqrt{1 + x(2-x)}} T_{3}\left(\sqrt{1 + x(2-x)}\right)dx
\]
where \( T_3(y) \) is the Chebyshev polynomial of degree 3.

### Step 1: Recall the Chebyshev Polynomial

\[
T_{3}(y) = 4y^{3} - 3y
\]

### Step 2: Let’s substitute \( y = \sqrt{1 + x(2-x)} \):

So
\[
T_3\left( \sqrt{1 + x(2-x)} \right ) = 4 \left ( 1 + x(2-x) \right )^{3/2} - 3 \sqrt{1 + x(2-x)}
\]

Thus, the integrand writes as:

\[
\frac{x^{-1/2}(2-x)^{-1/2}}{\sqrt{1 + x(2-x)}} \left[ 4(1 + x(2-x))^{3/2} - 3 (1 + x(2-x))^{1/2} \right ]
\]

This can be split into two integrals:

\[
I = 4 \int_{0}^{2} x^{-1/2} (2-x)^{-1/2} (1 + x(2-x)) \, dx - 3 \int_{0}^{2} x^{-1/2} (2-x)^{-1/2} dx
\]

### Step 3: Substitute \( x = 2 \sin^2 \theta \)

Let’s let \( x = 2 \sin^2 \theta \), so as \( x \) goes from \( 0 \) to \( 2 \), \( \theta \) goes from \( 0 \) to \( \pi/2 \):

- \( x = 2 \sin^2\theta \)
- \( dx = 4\sin\theta \cos\theta d\theta = 2\sin2\theta d\theta \)
- \( x^{-1/2} = (2 \sin^2 \theta)^{-1/2} = \frac{1}{\sqrt{2} \sin\theta} \)
- \( 2-x = 2(1 - \sin^2\theta) = 2\cos^2\theta \implies (2-x)^{-1/2} = \frac{1}{\sqrt{2} \cos\theta} \)
- \( x^{-1/2} (2-x)^{-1/2} = \frac{1}{2 \sin\theta \cos\theta} \)
- \( 1 + x(2-x) = 1 + 2 \sin^2\theta [2\cos^2\theta] = 1 + 4\sin^2\theta \cos^2\theta = 1 + \sin^2 2\theta \)

Now calculate:

- \( x^{-1/2} (2-x)^{-1/2} dx = \frac{1}{2 \sin\theta \cos\theta} \cdot 2\sin2\theta d\theta = \frac{2\sin2\theta}{2\sin\theta\cos\theta} d\theta = \frac{\sin2\theta}{\sin\theta\cos\theta} d\theta \)

Recall that \( \sin 2\theta = 2\sin\theta\cos\theta \), so:

\[
\frac{\sin2\theta}{\sin\theta\cos\theta} = 2
\]

Thus,
\[
x^{-1/2} (2-x)^{-1/2} dx = 2d\theta
\]

### Step 4: Rewrite the Integral

The limits become: when \( x=0 \), \( \theta=0 \), when \( x=2 \), \( \theta=\pi/2 \).

So
\[
I = 4 \int_{0}^{2} x^{-1/2} (2-x)^{-1/2} (1 + x(2-x)) dx - 3 \int_{0}^{2} x^{-1/2} (2-x)^{-1/2} dx
\]
\[
= 4 \int_{0}^{\pi/2} (1 + x(2-x)) \cdot 2 \, d\theta - 3 \int_{0}^{\pi/2} 2 \, d\theta
\]
\[
= 8 \int_{0}^{\pi/2} (1 + x(2-x)) d\theta - 6 \int_{0}^{\pi/2} d\theta
\]

Recall that
\[
x(2-x) = 2\sin^2\theta (2\cos^2\theta) = 4 \sin^2\theta \cos^2\theta = \sin^2 2\theta
\]
So,
\[
I = 8 \int_{0}^{\pi/2} (1 + \sin^2 2\theta) d\theta - 6 \left [ \theta \right ]_0^{\pi/2}
\]

\[
= 8 \int_{0}^{\pi/2} 1 d\theta + 8 \int_{0}^{\pi/2} \sin^2 2\theta d\theta - 6 \frac{\pi}{2}
\]

\[
= 8 \cdot \frac{\pi}{2} + 8 \int_{0}^{\pi/2} \sin^2 2\theta d\theta - 3\pi
\]

\[
= 4\pi + 8 \int_{0}^{\pi/2} \sin^2 2\theta d\theta - 3\pi
\]

\[
= \pi + 8 \int_{0}^{\pi/2} \sin^2 2\theta d\theta
\]

### Step 5: Compute \( \int_{0}^{\pi/2} \sin^2 2\theta d\theta \)

Recall that \( \sin^2 2\theta = \frac{1 - \cos 4\theta}{2} \):

\[
\int_{0}^{\pi/2} \sin^2 2\theta d\theta = \int_{0}^{\pi/2} \frac{1 - \cos 4\theta}{2} d\theta = \frac{1}{2} \int_{0}^{\pi/2} d\theta - \frac{1}{2} \int_{0}^{\pi/2} \cos 4\theta d\theta
\]

\[
= \frac{1}{2} \left [ \theta \right ]_{0}^{\pi/2} - \frac{1}{2} \left [ \frac{\sin 4\theta}{4}\right ]_0^{\pi/2}
\]
- \( \left [ \theta \right ]_{0}^{\pi/2} = \frac{\pi}{2} \)
- \( \sin 4\theta \) at \( \theta = \pi/2 \): \( \sin 4 \cdot \pi/2 = \sin 2\pi = 0 \)
- \( \sin 4\theta \) at \( \theta = 0 \): \( \sin 0 = 0 \)
So \( \left [ \frac{\sin 4\theta}{4} \right ]_{0}^{\pi/2} = 0 \)

Thus,
\[
\int_{0}^{\pi/2} \sin^2 2\theta d\theta = \frac{1}{2} \cdot \frac{\pi}{2} = \frac{\pi}{4}
\]

### Final Step: Plug in

So,
\[
I = \pi + 8 \cdot \frac{\pi}{4} = \pi + 2\pi = 3\pi
\]

### Step 6: Numerical evaluation

\[
3\pi \approx 9.4247779607
\]

### JSON Output

```json
{"answer": "3\\pi", "numerical_answer": "9.4247779607"}
```