# Evaluating $\int\limits_{0}^{2}x^{1/4}(2-x)^{-1/4}\cosh\left(\sqrt[4]{x(2-x)}\right)dx$

## Step 1: Make a substitution

Looking at the structure of the integral, I'll try a substitution that simplifies both the radical expressions and the hyperbolic cosine.

Let's try $t = \sqrt[4]{x(2-x)}$. To find $dx$ in terms of $t$, I need to determine the relationship between $x$ and $t$.

First, $t^4 = x(2-x) = 2x - x^2$

This means $x^2 - 2x + t^4 = 0$

Using the quadratic formula:
$x = \frac{2 \pm \sqrt{4-4t^4}}{2} = 1 \pm \sqrt{1-t^4}$

Since $x$ ranges from 0 to 2, we need to use both solutions:
- When $x$ goes from 0 to 1, we use $x = 1 - \sqrt{1-t^4}$
- When $x$ goes from 1 to 2, we use $x = 1 + \sqrt{1-t^4}$

From the limits, when $x = 0$, $t = 0$, and when $x = 2$, $t = 0$.
When $x = 1$, $t = 1$.

## Step 2: Compute the differential

For $x = 1 - \sqrt{1-t^4}$:
$\frac{dx}{dt} = \frac{4t^3}{2\sqrt{1-t^4}}$

For $x = 1 + \sqrt{1-t^4}$:
$\frac{dx}{dt} = -\frac{4t^3}{2\sqrt{1-t^4}}$

## Step 3: Express the original terms in terms of $t$

For the first part (0 to 1):
$x^{1/4} = (1 - \sqrt{1-t^4})^{1/4}$
$(2-x)^{-1/4} = (2-(1 - \sqrt{1-t^4}))^{-1/4} = (1 + \sqrt{1-t^4})^{-1/4}$

For the second part (1 to 2):
$x^{1/4} = (1 + \sqrt{1-t^4})^{1/4}$
$(2-x)^{-1/4} = (2-(1 + \sqrt{1-t^4}))^{-1/4} = (1 - \sqrt{1-t^4})^{-1/4}$

## Step 4: Simplification using symmetry

Due to the symmetry of the problem around $x = 1$, the integral from 0 to 1 equals the integral from 1 to 2. Therefore:

$\int\limits_{0}^{2}x^{1/4}(2-x)^{-1/4}\cosh\left(\sqrt[4]{x(2-x)}\right)dx = 2\int\limits_{0}^{1}x^{1/4}(2-x)^{-1/4}\cosh\left(\sqrt[4]{x(2-x)}\right)dx$

## Step 5: Apply substitution formula

With our substitution $t = \sqrt[4]{x(2-x)}$, the integral becomes:

$2\int\limits_{0}^{1}\cosh(t) \cdot 2t \cdot dt = 4\int\limits_{0}^{1}t\cosh(t)dt$

## Step 6: Integrate $t\cosh(t)$

Using integration by parts with $u = t$ and $dv = \cosh(t)dt$:
$\int t\cosh(t)dt = t\sinh(t) - \int \sinh(t)dt = t\sinh(t) - \cosh(t) + C$

## Step 7: Evaluate the definite integral

$4\int\limits_{0}^{1}t\cosh(t)dt = 4[t\sinh(t) - \cosh(t)]_0^1$
$= 4[\sinh(1) - \cosh(1) + 1]$
$= 4\sinh(1) - 4\cosh(1) + 4$

## Step 8: Calculate the numerical value

$\sinh(1) \approx 1.1752011936438014$
$\cosh(1) \approx 1.5430806348152437$

$4\sinh(1) - 4\cosh(1) + 4 = 4 \cdot 1.1752011936438014 - 4 \cdot 1.5430806348152437 + 4$
$= 4.7008047745752056 - 6.1723225392609748 + 4$
$= 2.5284822353142308$

## Final answer

The exact result is $4\sinh(1) - 4\cosh(1) + 4$

The numerical approximation is $2.5284822353$ (rounded to 10 decimal places)

{"answer": "4\\sinh(1) - 4\\cosh(1) + 4", "numerical_answer": "2.5284822353"}