# Evaluating $\int_{\frac{1}{4}}^{4}\frac{\tan^{-1}(x)}{x}\,\mathrm{d}x$

Let's compute this definite integral analytically.

## Step 1: Substitution
Let's use the substitution $u = \frac{1}{x}$ to simplify the integral.

When $x = \frac{1}{4}$, $u = 4$
When $x = 4$, $u = \frac{1}{4}$

Also, $dx = -\frac{1}{u^2}du$

Using the property $\tan^{-1}(x) + \tan^{-1}\left(\frac{1}{x}\right) = \frac{\pi}{2}$ for $x > 0$, we have:
$\tan^{-1}(x) = \frac{\pi}{2} - \tan^{-1}\left(\frac{1}{x}\right) = \frac{\pi}{2} - \tan^{-1}(u)$

Substituting into the integral:
$\int_{\frac{1}{4}}^{4}\frac{\tan^{-1}(x)}{x}\,\mathrm{d}x = \int_{4}^{\frac{1}{4}}\frac{\frac{\pi}{2} - \tan^{-1}(u)}{1/u}\left(-\frac{1}{u^2}\right)\,\mathrm{d}u$

Simplifying:
$= \int_{4}^{\frac{1}{4}}\left(\frac{\pi}{2} - \tan^{-1}(u)\right)\left(-\frac{1}{u}\right)\,\mathrm{d}u$
$= \int_{\frac{1}{4}}^{4}\left(\frac{\pi}{2} - \tan^{-1}(u)\right)\frac{1}{u}\,\mathrm{d}u$

So we have:
$\int_{\frac{1}{4}}^{4}\frac{\tan^{-1}(x)}{x}\,\mathrm{d}x = \int_{\frac{1}{4}}^{4}\frac{\frac{\pi}{2} - \tan^{-1}(u)}{u}\,\mathrm{d}u$
$= \int_{\frac{1}{4}}^{4}\frac{\frac{\pi}{2}}{u}\,\mathrm{d}u - \int_{\frac{1}{4}}^{4}\frac{\tan^{-1}(u)}{u}\,\mathrm{d}u$

Observe that we've arrived at the same integral, but with different bounds. Let's use this insight.

## Step 2: Leveraging the Symmetry
We have:
$\int_{\frac{1}{4}}^{4}\frac{\tan^{-1}(x)}{x}\,\mathrm{d}x = \int_{\frac{1}{4}}^{4}\frac{\frac{\pi}{2}}{x}\,\mathrm{d}x - \int_{\frac{1}{4}}^{4}\frac{\tan^{-1}(x)}{x}\,\mathrm{d}x$

Rearranging:
$2\int_{\frac{1}{4}}^{4}\frac{\tan^{-1}(x)}{x}\,\mathrm{d}x = \int_{\frac{1}{4}}^{4}\frac{\frac{\pi}{2}}{x}\,\mathrm{d}x$
$= \frac{\pi}{2}\int_{\frac{1}{4}}^{4}\frac{1}{x}\,\mathrm{d}x$
$= \frac{\pi}{2}[\ln|x|]_{\frac{1}{4}}^{4}$
$= \frac{\pi}{2}[\ln(4) - \ln(\frac{1}{4})]$
$= \frac{\pi}{2}[\ln(4) + \ln(4)]$
$= \frac{\pi}{2} \cdot 2\ln(4)$
$= \pi\ln(4)$

Therefore:
$\int_{\frac{1}{4}}^{4}\frac{\tan^{-1}(x)}{x}\,\mathrm{d}x = \frac{\pi\ln(4)}{2}$

## Step 3: Final Result
We can simplify further:
$\frac{\pi\ln(4)}{2} = \frac{\pi\ln(2^2)}{2} = \frac{\pi \cdot 2\ln(2)}{2} = \pi\ln(2)$

Therefore, the exact answer is $\pi\ln(2)$.

## Step 4: Numerical Approximation
$\pi\ln(2) \approx 3.14159265359 \times 0.693147180560 \approx 2.1775860903$

{"answer": "\\pi\\ln(2)", "numerical_answer": "2.1775860903"}