Given:
\[
\int_0^{2.0}x^{-1.0/4}(2.0-x)^{-(1.0+2)/4}I_1.0\left(1.0\sqrt[4]{x(2.0-x)}\right)dx
\]

Substitute for parameters:

- \(x^{-1.0/4} = x^{-1/4}\)
- \(2.0-x\)
- Exponent: \(-(1.0+2)/4 = -3/4\)
- \(I_1.0(\cdots)\) is the modified Bessel function of the first kind.

So rewrite as:
\[
\int_0^2 x^{-1/4}(2-x)^{-3/4} I_1\left((x(2-x))^{1/4}\right) dx
\]

Let us try substitution and use an integral formula.

### Step 1: Substitution

Let \(x = 2 \sin^2\theta\), \(x \in [0,2]\) means \(\theta \in [0, \pi/2]\):

- \(dx = 4 \sin\theta \cos\theta d\theta = 2\sin(2\theta)d\theta\)
- \(2 - x = 2\cos^2\theta\)
- \(x(2-x) = 4\sin^2\theta \cos^2\theta = (\sin 2\theta)^2\)
- \((x(2-x))^{1/4} = \sin^{1/2} 2\theta\)

Now,
\[
x^{-1/4} = (2\sin^2\theta)^{-1/4} = 2^{-1/4}\sin^{-1/2}\theta
\]
\[
(2-x)^{-3/4} = (2\cos^2\theta)^{-3/4} = 2^{-3/4}\cos^{-3/2}\theta
\]

So,
\[
\int_0^{\pi/2}
2^{-1/4}\sin^{-1/2}\theta \cdot 2^{-3/4}\cos^{-3/2}\theta
\cdot I_1\left(\sin^{1/2} 2\theta\right) \cdot 2\sin 2\theta d\theta
\]

Combine constants:
\[
2^{-1/4} \cdot 2^{-3/4} \cdot 2 = 2^{-1} \cdot 2 = 1
\]

And \(\sin 2\theta = 2\sin\theta\cos\theta\), so:
\[
\sin 2\theta d\theta
\]

So, combining everything:
\[
\int_0^{\pi/2} \sin^{-1/2}\theta \cos^{-3/2}\theta \cdot I_1\left(\sin^{1/2} 2\theta\right) \cdot \sin 2\theta d\theta
\]

But:
- \(\sin 2\theta = 2\sin\theta\cos\theta\)

So:
\[
\sin^{-1/2}\theta \cos^{-3/2}\theta \cdot \sin 2\theta = 2 \sin^{-1/2+1}\theta \cos^{-3/2+1}\theta = 2 \sin^{1/2}\theta \cos^{-1/2}\theta
\]

So the integral becomes:
\[
2 \int_0^{\pi/2} \sin^{1/2}\theta \cos^{-1/2}\theta \cdot I_1\left(\sin^{1/2} 2\theta\right) d\theta
\]

### Step 2: Further Substitution

Let \(u = \sin 2\theta\), \(du = 2\cos 2\theta d\theta\).

But with exponents, it's likely best to look for a known integral.

#### Let's revisit the original integral:

Recall a tabulated result:
\[
\int_0^a x^{\mu - 1}(a - x)^{\nu - 1} I_p\left(2b \sqrt{x(a-x)}\right) dx = \frac{\Gamma(\mu)\Gamma(\nu)}{2\Gamma(\mu+\nu)} a^{\mu + \nu - 1} \left[b a \right]^p I_{\mu+\nu+p-1}(b a)
\]
where the exponents and argument match up, possibly after a change of argument.

But our integral is:
\[
\int_0^2 x^{\alpha - 1} (2-x)^{\beta - 1} I_1 \left( (x(2-x))^{1/4} \right) dx
\]
Let's try to match:

Set
- \(a = 2\)
- The Bessel function should take the form \(I_p(2b \sqrt{x(a-x)})\), but ours is \(I_1\left((x(2-x))^{1/4}\right)\).
- Set \(2b \sqrt{x(a-x)} = (x(2-x))^{1/4}\)
- So \(2b \sqrt{x(a-x)} = (x(a-x))^{1/4}\) â‡’ Only possible if \(x(a-x) \geq 0\), which is true for \(x \in [0,a]\).

Thus, the argument is different; but let's try \(I_1\left( \lambda (x(a-x))^{1/4} \right)\).

Alternatively, consider expanding the Bessel function definition:

\[
I_1(z) = \sum_{k=0}^\infty \frac{(z/2)^{2k+1}}{k! \Gamma(k+2)}
\]
Let \(z = (x(2-x))^{1/4}\):

So,
\[
I_1\left((x(2-x))^{1/4}\right) = \sum_{k=0}^{\infty} \frac{1}{k! \Gamma(k+2)} \left(\frac{(x(2-x))^{1/4}}{2}\right)^{2k+1}
\]
\[
= \sum_{k=0}^{\infty} \frac{1}{k! \Gamma(k+2) 2^{2k+1}} \left((x(2-x))^{1/4}\right)^{2k+1}
\]
\[
= \sum_{k=0}^{\infty} \frac{1}{k! \Gamma(k+2) 2^{2k+1}} (x(2-x))^{(2k+1)/4}
\]

Plug this into the original integral:

\[
\int_0^2 x^{-1/4}(2-x)^{-3/4} \sum_{k=0}^\infty \frac{1}{k! \Gamma(k+2) 2^{2k+1}} (x(2-x))^{(2k+1)/4} dx
\]
\[
= \sum_{k=0}^{\infty} \frac{1}{k! \Gamma(k+2) 2^{2k+1}} \int_0^2 x^{-1/4} (2-x)^{-3/4} (x(2-x))^{(2k+1)/4} dx
\]
\[
= \sum_{k=0}^{\infty} \frac{1}{k! \Gamma(k+2) 2^{2k+1}} \int_0^2 x^{-1/4 + (2k+1)/4} (2-x)^{-3/4 + (2k+1)/4} dx
\]
\[
= \sum_{k=0}^\infty \frac{1}{k! \Gamma(k+2) 2^{2k+1}} \int_0^2 x^{(2k)/4} (2-x)^{(2k-2)/4} dx
\]

So \(x^{k/2}\) and \((2-x)^{(k-1)/2}\).

Let us write:
\[
x^{k/2} (2-x)^{(k-1)/2}
\]

Now, let \(u = x/2\), \(x = 2u\), \(dx = 2 du\), \(u \in [0,1]\):

- \(x^{k/2} = (2u)^{k/2} = 2^{k/2} u^{k/2}\)
- \(2-x = 2(1-u)\), so \((2-x)^{(k-1)/2} = [2(1-u)]^{(k-1)/2} = 2^{(k-1)/2} (1-u)^{(k-1)/2}\)
- \(dx = 2 du\)

Integral becomes:
\[
\int_0^1 2^{k/2} u^{k/2} \cdot 2^{(k-1)/2} (1-u)^{(k-1)/2} \cdot 2 du
\]
\[
= 2^{k/2 + (k-1)/2 + 1} \int_0^1 u^{k/2} (1-u)^{(k-1)/2} du
\]
\[
k/2 + (k-1)/2 + 1 = (k + k - 1)/2 + 1 = (2k - 1)/2 + 1 = (2k + 1)/2
\]
So the constant is \(2^{(2k+1)/2}\).

So,
\[
2^{(2k+1)/2} \int_0^1 u^{k/2} (1-u)^{(k-1)/2} du
\]
This is a Beta function:
\[
\int_0^1 u^{p-1}(1-u)^{q-1} du = B(p, q) = \frac{\Gamma(p)\Gamma(q)}{\Gamma(p+q)}
\]
Here, \(p = k/2 + 1\), \(q = (k-1)/2 + 1 = (k+1)/2\):

Therefore, the integral is:
\[
\int_0^2 x^{k/2}(2-x)^{(k-1)/2} dx = 2^{(2k+1)/2} B\left(k/2+1, (k+1)/2\right)
\]

Return to our sum:
\[
\sum_{k=0}^\infty \frac{1}{k! \Gamma(k+2) 2^{2k+1}} \cdot 2^{(2k+1)/2} B\left(\frac{k}{2}+1, \frac{k+1}{2}\right)
\]
\[
= \sum_{k=0}^\infty \frac{1}{k! \Gamma(k+2)} 2^{-2k-1 + (2k+1)/2} B\left(\frac{k}{2}+1, \frac{k+1}{2}\right)
\]
\[
2^{-2k-1 + (2k+1)/2} = 2^{-2k -1} 2^{(2k+1)/2} = 2^{(-2k-1)+(2k+1)/2} = 2^{(-2k-1+2k/2+1/2)} = 2^{(-2k+2k/2-1+1/2)} = 2^{(-2k+ k-1+0.5)}=2^{(-k-0.5)} = \frac{1}{2^{k}\sqrt{2}}
\]

Thus, the answer is:
\[
\sum_{k=0}^\infty \frac{B\left(\frac{k}{2}+1, \frac{k+1}{2}\right)}{k! \Gamma(k+2) 2^{k}\sqrt{2}}
\]

Recall \( B(p,q) = \frac{\Gamma(p)\Gamma(q)}{\Gamma(p+q)} \), \( \Gamma(k+2) = (k+1)! \).

So
\[
B\left(\frac{k}{2}+1, \frac{k+1}{2}\right) = \frac{\Gamma\left(\frac{k}{2}+1\right)\Gamma\left(\frac{k+1}{2}\right)}{\Gamma\left(\frac{k}{2}+1 + \frac{k+1}{2}\right)}
= \frac{\Gamma\left(\frac{k}{2}+1\right)\Gamma\left(\frac{k+1}{2}\right)}{\Gamma(k+\frac{3}{2})}
\]
Because
\[
\frac{k}{2}+1 + \frac{k+1}{2} = \frac{k+2+k+1}{2} = \frac{2k+3}{2} = k + \frac{3}{2}
\]

Collecting everything, the answer is:

\[
\boxed{
\int_0^2 x^{-1/4}(2-x)^{-3/4} I_1\left((x(2-x))^{1/4}\right)dx
= \frac{1}{\sqrt{2}} \sum_{k=0}^\infty \frac{\Gamma\left(\frac{k}{2}+1\right)\Gamma\left(\frac{k+1}{2}\right)}{k! (k+1)! 2^{k} \Gamma\left(k+\frac{3}{2}\right)}
}
\]

---

### Step 3: Numerical Evaluation

Compute the first several terms:

Let us do this for \( k = 0, 1, 2, 3, 4 \):

#### For \(k=0\):

- \( \frac{k}{2}+1 = 1 \), \( \Gamma(1) = 1 \)
- \( \frac{k+1}{2} = 0.5 \), \( \Gamma(0.5) = \sqrt{\pi} \)
- \( \Gamma\left(0 + \frac{3}{2}\right) = \Gamma(1.5) = \frac{1}{2}\sqrt{\pi} \)
- \( k! = 1, (k+1)! = 1 \)
- \( 2^{k} = 1 \)
- So numerator: \( 1 \cdot \sqrt{\pi} \)
- Denominator: \( 1 \cdot 1 \cdot 1 \cdot \frac{1}{2}\sqrt{\pi} = \frac{1}{2}\sqrt{\pi} \)
- So, term is: \( \frac{1}{\sqrt{2}} \cdot \frac{1 \times \sqrt{\pi}}{\frac{1}{2}\sqrt{\pi}} = \frac{1}{\sqrt{2}} \cdot 2 = \sqrt{2} \approx 1.4142135624 \)

#### For \(k=1\):

- \( \frac{1}{2} + 1 = 1.5 \), \( \Gamma(1.5) = 0.5\sqrt{\pi} \)
- \( \frac{2}{2} = 1 \), \( \Gamma(1) = 1 \)
- \( k+1 = 2, (k+1)! = 2 \)
- \( 2^{1} = 2 \)
- \( \Gamma(2.5) = (1.5)\Gamma(1.5) = 1.5 \times 0.5\sqrt{\pi} = 0.75\sqrt{\pi} \)
- Numerator: \( 0.5\sqrt{\pi} \)
- Denominator: \( 1 \cdot 2 \cdot 2 \cdot 0.75\sqrt{\pi} = 3\sqrt{\pi} \)
- Combined: \( \frac{1}{\sqrt{2}} \cdot \frac{0.5\sqrt{\pi}}{3\sqrt{\pi}} = \frac{1}{\sqrt{2}} \cdot \frac{0.5}{3} = \frac{1}{\sqrt{2}} \cdot 0.1666666667 \approx 0.1178511302 \)

#### For \(k=2\):

- \( 1 + 1 = 2 \), \( \Gamma(2) = 1 \)
- \( 1.5 + 1 = 2.5 \), \( \Gamma(1.5) = 0.5\sqrt{\pi} \)
- \( k! = 2, (k+1)! = 3 \), \( 2^{2} = 4 \)
- \( \Gamma(3.5) = 2.5 \cdot 1.329340388 = 3.32335097 \), but better to do recursively: \( \Gamma(3.5) = (2.5)(1.329340388) = 3.32335097 \)
But let's use \( \Gamma(3.5) = (2.5) \Gamma(2.5) \), \( \Gamma(2.5) = 1.329340388 \); so \( \Gamma(3.5) = 3.32335097 \)
- Numerator: \( 1 \cdot 0.5\sqrt{\pi} = 0.5\sqrt{\pi} \)
- Denominator: \( 2 \cdot 3 \cdot 4 \cdot 3.32335097 \)
First, \( 2 \cdot 3 = 6 \), \( 6 \cdot 4 = 24 \), denominator \( = 24 \cdot 3.32335097 = 79.7604233 \)

Wait, but we missed \( \sqrt{\pi} \) in the denominator? Let's be careful.

- For the Beta function: \( \Gamma(2) = 1, \Gamma(1.5) = 0.886226925 \)
- \( \Gamma(3.5) = 3.323350970 \)
So numerator: \( 1 \cdot 0.886226925 = 0.886226925 \)
Denominator: \( 2 \cdot 3 \cdot 4 \cdot 3.323350970 = 24 \cdot 3.323350970 = 79.76042328 \)

So term: \( \frac{0.886226925}{79.76042328} = 0.0111139617 \)

So with the prefactor \( \frac{1}{\sqrt{2}} = 0.7071067812 \):
\( 0.0111139617 \times 0.7071067812 = 0.0078626681 \)

#### For \(k=3\):

- \( 1.5 + 1 = 2.5 \), \( \Gamma(2.5) = 1.329340388 \)
- \( (k+1)/2 = 2 \), \( \Gamma(2) = 1 \)
- \( k! = 6, (k+1)! = 24 \), \( 2^{3} = 8 \)
- \( \Gamma(4.5) = 3.5 \Gamma(3.5) = 3.5 \times 3.323350970 = 11.63172840 \)
- Numerator: \( 1.329340388 \times 1 = 1.329340388 \)
- Denominator: \( 6 \cdot 24 \cdot 8 \cdot 11.63172840 \)
First, \( 6 \cdot 24 = 144 \), \( 144 \cdot 8 = 1152 \), \( 1152 \times 11.63172840 = 13,406.15497 \)
Now term: \( 1.329340388 / 13,406.15497 = 0.0000991798 \)
With the prefactor \( 0.7071067812 \): \( 0.0000991798 \cdot 0.7071067812 = 0.0000701308 \)

#### For \( k=4 \):

- \( 2 + 1 = 3 \), \( \Gamma(3) = 2 \)
- \( 2.5 + 1 = 3.5 \), \( \Gamma(3.5) = 3.323350970 \)
- \( k! = 24, (k+1)! = 120 \), \( 2^{4} = 16 \)
- \( \Gamma(5.5) = 4.5 \Gamma(4.5) = 4.5 \times 11.63172840 = 52.3427778 \)
- Numerator: \( 2 \times 3.323350970 = 6.64670194 \)
- Denominator: \( 24 \cdot 120 = 2880, 2880 \cdot 16 = 46,080, 46,080 \cdot 52.3427778 = 2,411,395.84 \)
Thus, term: \( 6.64670194 / 2,411,395.84 = 0.0000027555 \)
With the prefactor: \( 0.0000027555 \times 0.7071067812 = 0.0000019485 \)

Summing up:

- \( k=0 \): \( 1.4142135624 \)
- \( k=1 \): \( 0.1178511302 \)
- \( k=2 \): \( 0.0078626681 \)
- \( k=3 \): \( 0.0000701308 \)
- \( k=4 \): \( 0.0000019485 \)

Sum: \( 1.4142135624 + 0.1178511302 + 0.0078626681 + 0.0000701308 + 0.0000019485 = 1.4399980599 \)

Note how quickly the terms decrease. The sum will not change much for more terms. Let's estimate up to 10 terms for safety.

If we sum more terms, the next term at \(k=5\) will be perhaps \(10^{-8}\), so the sum to 10 terms will differ at the <6th decimal place.

Therefore, we have:

\[
\boxed{1.4399980599}
\]

Rounded to 10 decimal places: **1.4399980599**

---

## Final Answer (JSON)

```json
{"answer": "\\frac{1}{\\sqrt{2}} \\sum_{k=0}^\\infty \\frac{\\Gamma\\left(\\frac{k}{2}+1\\right)\\Gamma\\left(\\frac{k+1}{2}\\right)}{k!\\,(k+1)!\\,2^{k}\\,\\Gamma\\left(k+\\frac{3}{2}\\right)}", "numerical_answer": "1.4399980599"}
```