We start with the integral

  I = ∫₀² x^(–1/2) (2 – x)^(–1/2) cosh(√(x(2 – x))) dx.

Step 1. Substitution

Let
  x = 1 – cos θ. 
Then when x = 0 we have 1 – cos θ = 0 ⟹ cos θ = 1 ⟹ θ = 0, 
and when x = 2 we have 1 – cos θ = 2 ⟹ cos θ = –1 ⟹ θ = π.
Also, differentiate:
  dx = sin θ dθ.

Now compute the factors in the integrand:

• x^(–½) and (2–x)^(–½): Note that
  x = 1 – cos θ and 2 – x = 2 – (1 – cos θ) = 1 + cos θ.
Thus,
  x(2 – x) = (1 – cos θ)(1 + cos θ) = 1 – cos²θ = sin²θ,
and so
  √(x(2 – x)) = |sin θ| = sin θ  (since 0 ≤ θ ≤ π, where sin θ ≥ 0).

Also,
  x^(–½)(2 – x)^(–½) = 1/√[(1–cosθ)(1+cosθ)] = 1/sin θ.

Step 2. Transforming the integral

Substitute all pieces into the original integral:

  I = ∫₀π [1/sin θ] · cosh( sin θ ) · (sin θ dθ)
     = ∫₀π cosh(sin θ) dθ.

Thus the integral simplifies to

  I = ∫₀π cosh(sin θ) dθ.

Step 3. Expressing the Integral via Bessel Functions

A very neat trick is to express cosh(sin θ) in terms of a cosine series. Notice that
  cosh(sin θ) = cos(i sin θ)
and we can use the Jacobi–Anger expansion for the cosine:
  cos(z sin θ) = J₀(z) + 2 Σₙ₌₁∞ J₂ₙ(z) cos(2nθ),
with z replaced by i. Using the relation
  J₂ₙ(i) = i^(2n) I₂ₙ(1) = (–1)ⁿ I₂ₙ(1),
we have
  cosh(sin θ) = J₀(i) + 2 Σₙ₌₁∞ (–1)ⁿ I₂ₙ(1) cos(2nθ).

When we integrate from 0 to π, the cosine terms (for n ≥ 1) have zero average:
  ∫₀π cos(2nθ) dθ = 0 for n ≥ 1.
Thus only the n = 0 term contributes. Note also that
  J₀(i) = I₀(1)
(the modified Bessel function of order zero).

Hence,
  I = ∫₀π cosh(sin θ) dθ = π J₀(i) = π I₀(1).

Step 4. Final Answer and Numerical Approximation

Thus the exact answer is:
  I = π I₀(1).

Using the approximate value I₀(1) ≈ 1.2660658777520082 and π ≈ 3.141592653589793, we have
  I ≈ 3.141592653589793 × 1.2660658777520082 ≈ 3.9764027280.

The final answer in the required JSON format is:
{"answer": "\\pi I_0(1)", "numerical_answer": "3.9764027280"}