Let's solve the integral:
\[
I = \int_1^{e^e} \frac{\log\left(x^{\log(x^x)}\right)}{x^2} \, dx
\]

**Step 1: Simplify the integrand**

First, simplify \(\log\left(x^{\log(x^x)}\right)\):

- \(\log(x^x) = x \log x\)
- So, \(x^{\log(x^x)} = x^{x \log x}\)
- \(\log\left(x^{x \log x}\right) = x \log x \cdot \log x = x (\log x)^2\)

So the integrand becomes:
\[
\frac{\log\left(x^{\log(x^x)}\right)}{x^2} = \frac{x (\log x)^2}{x^2} = \frac{(\log x)^2}{x}
\]

Our integral is now:
\[
I = \int_1^{e^e} \frac{(\log x)^2}{x} \, dx
\]

**Step 2: Integrate analytically**

Recall that:
\[
\int \frac{(\log x)^n}{x} \, dx = \frac{(\log x)^{n+1}}{n+1} + C
\]
For \(n = 2\):
\[
\int \frac{(\log x)^2}{x} \, dx = \frac{(\log x)^3}{3} + C
\]

Thus,
\[
I = \left. \frac{(\log x)^3}{3} \right|_1^{e^e}
\]
Calculate at the bounds:

- At \(x = e^e\): \(\log(e^e) = e\), so \((\log(e^e))^3 = e^3\)
- At \(x = 1\): \(\log(1) = 0\), so \((\log 1)^3 = 0\)

So:
\[
I = \frac{1}{3} (e^3 - 0) = \frac{e^3}{3}
\]

**Step 3: Numerical approximation**

Compute \(e^3 \approx (2.718281828459045)^3\):

\[
e^3 \approx 20.0855369232
\]
So,
\[
I \approx \frac{20.0855369232}{3} \approx 6.6951789744
\]

**Step 4: Format as JSON**

```json
{"answer": "\\frac{e^3}{3}", "numerical_answer": "6.6951789744"}
```