<think>
Okay, so I need to compute the definite integral from 0 to π/4 of ln(cot x - 1) dx. Hmm, let's start by understanding the integrand. The natural logarithm of cotangent x minus 1. Cot x is cos x over sin x, right? So maybe I can rewrite cot x - 1 as (cos x - sin x)/sin x. But I'm not sure if that helps immediately.

Wait, maybe a substitution would work here. Let me think. The integral is ∫₀^{π/4} ln(cot x - 1) dx. Let's consider substitution to simplify the expression inside the logarithm. Let me set t = x, but that's not helpful. Maybe a substitution that relates to the argument of the logarithm. Let's see, cot x - 1. Alternatively, perhaps using a trigonometric identity. Let me recall that cot x = tan(π/2 - x). So cot x - 1 = tan(π/2 - x) - 1. Not sure if that helps.

Alternatively, maybe express cot x in terms of sin and cos. So cot x = cos x / sin x. Then cot x - 1 = (cos x - sin x)/sin x. So ln(cot x - 1) = ln(cos x - sin x) - ln(sin x). Hmm, splitting the logarithm into two terms. So the integral becomes ∫ ln(cos x - sin x) dx - ∫ ln(sin x) dx, both from 0 to π/4.

Wait, but integrating ln(sin x) from 0 to π/4 is a known integral? I remember that the integral of ln(sin x) from 0 to π/2 is - (π/2) ln 2. But here the limits are 0 to π/4. Maybe there's a known result for that. Let me check. The integral of ln(sin x) from 0 to a can be expressed using the formula involving the dilogarithm function, but maybe there's a way to relate it here.

Alternatively, perhaps integrating by parts. Let me try integrating ln(cot x - 1) directly. Let u = ln(cot x - 1), dv = dx. Then du would be [ -csc²x / (cot x - 1) ] dx, and v = x. Hmm, but integrating by parts might complicate things further. Let me see:

∫ ln(cot x - 1) dx = x ln(cot x - 1) - ∫ x * [ -csc²x / (cot x - 1) ] dx.

But this seems messy. Maybe another substitution. Let me try substituting t = π/4 - x. Because the upper limit is π/4, so when x = 0, t = π/4, and when x = π/4, t = 0. So the integral becomes ∫_{π/4}^0 ln(cot(π/4 - t) - 1) (-dt) = ∫₀^{π/4} ln(cot(π/4 - t) - 1) dt.

Now, cot(π/4 - t) is (cos(π/4 - t))/(sin(π/4 - t)). Using the identity cot(A - B) = (cot A cot B + 1)/(cot B - cot A), but maybe it's easier to compute directly. Let's compute cot(π/4 - t):

cot(π/4 - t) = [cos(π/4)cos t + sin(π/4)sin t] / [sin(π/4)cos t - cos(π/4)sin t] = [ (√2/2)(cos t + sin t) ] / [ (√2/2)(cos t - sin t) ] = (cos t + sin t)/(cos t - sin t).

So cot(π/4 - t) - 1 = [ (cos t + sin t)/(cos t - sin t) ] - 1 = [ (cos t + sin t) - (cos t - sin t) ] / (cos t - sin t) = [2 sin t] / (cos t - sin t).

Therefore, ln(cot(π/4 - t) - 1) = ln(2 sin t) - ln(cos t - sin t). So the integral becomes ∫₀^{π/4} [ln(2 sin t) - ln(cos t - sin t)] dt.

But the original integral was ∫₀^{π/4} ln(cot x -1) dx, which after substitution becomes the same as this. Let me denote the original integral as I. Then, I = ∫₀^{π/4} [ln(2 sin t) - ln(cos t - sin t)] dt. But this seems like we can relate it back to the original integral. Let's see:

I = ∫₀^{π/4} ln(2 sin t) dt - ∫₀^{π/4} ln(cos t - sin t) dt.

But the second integral here is similar to the original integrand. Wait, in the original integral, we had ln(cot x -1) dx, which we split into ln(cos x - sin x) - ln(sin x). So maybe combining these two expressions for I?

Wait, let's recap. The original integral I is equal to:

I = ∫₀^{π/4} [ln(cos x - sin x) - ln(sin x)] dx.

But after substitution, we have:

I = ∫₀^{π/4} [ln(2 sin t) - ln(cos t - sin t)] dt.

So substituting variables back to x (since t is a dummy variable), we can write:

I = ∫₀^{π/4} ln(2 sin x) dx - ∫₀^{π/4} ln(cos x - sin x) dx.

But from the original expression, I = ∫ [ln(cos x - sin x) - ln(sin x)] dx. So:

I = ∫ ln(cos x - sin x) dx - ∫ ln(sin x) dx.

Comparing the two expressions for I:

From substitution: I = ∫ ln(2 sin x) dx - ∫ ln(cos x - sin x) dx.

So:

I = ∫ ln(2) dx + ∫ ln(sin x) dx - ∫ ln(cos x - sin x) dx.

But from the original expression, I = ∫ ln(cos x - sin x) dx - ∫ ln(sin x) dx.

So setting these equal:

∫ ln(cos x - sin x) dx - ∫ ln(sin x) dx = ∫ ln(2) dx + ∫ ln(sin x) dx - ∫ ln(cos x - sin x) dx.

Bringing all terms to one side:

2 ∫ ln(cos x - sin x) dx - 2 ∫ ln(sin x) dx - ∫ ln(2) dx = 0.

But this seems complicated. Maybe instead, adding the two expressions for I. Wait, perhaps adding the original I and the substituted I.

Original I: I = A - B, where A = ∫ ln(cos x - sin x) dx, B = ∫ ln(sin x) dx.

Substituted I: I = ∫ ln(2 sin x) dx - A = ln(2) * (π/4) + B - A.

So:

Original I = A - B.

Substituted I = (π/4) ln 2 + B - A.

Therefore, setting them equal:

A - B = (π/4) ln 2 + B - A.

Bringing terms together:

A - B - B + A = (π/4) ln 2.

2A - 2B = (π/4) ln 2.

Divide both sides by 2:

A - B = (π/8) ln 2.

But A - B is the original integral I. Therefore, I = (π/8) ln 2.

Wait, that's a result! So the integral I equals π/8 times ln 2. But let me verify this because the steps might have a mistake.

Let me recap:

We started with I = ∫₀^{π/4} ln(cot x -1) dx.

Expressed as I = ∫ [ln(cos x - sin x) - ln(sin x)] dx = A - B.

Then, using substitution t = π/4 - x, we found that I = ∫ [ln(2 sin x) - ln(cos x - sin x)] dx = (π/4) ln 2 + B - A.

So setting I = A - B and I = (π/4) ln 2 + B - A.

Therefore:

A - B = (π/4) ln 2 + B - A.

Bringing A terms to left and B terms to right:

A + A = (π/4) ln 2 + B + B.

2A = (π/4) ln 2 + 2B.

Then, 2A - 2B = (π/4) ln 2.

Divide by 2: A - B = (π/8) ln 2.

But A - B is I, so I = (π/8) ln 2.

Therefore, the integral equals π/8 times ln 2. Wait, but π/8 multiplied by ln 2? Let me check the substitution steps again.

Wait, when we did the substitution t = π/4 - x, then dt = -dx, so the integral becomes ∫_{π/4}^0 ln(cot(π/4 - t) -1) (-dt) = ∫₀^{π/4} ln(cot(π/4 - t) -1) dt.

Then, we found that cot(π/4 - t) -1 = 2 sin t / (cos t - sin t). So ln(cot(π/4 - t) -1) = ln(2 sin t) - ln(cos t - sin t). Therefore, the integral becomes ∫₀^{π/4} [ln(2 sin t) - ln(cos t - sin t)] dt. Which is ln(2) * (π/4) + ∫ ln(sin t) dt - ∫ ln(cos t - sin t) dt. So that's ln(2) * (π/4) + B - A. Therefore, I = (π/4) ln 2 + B - A.

But original I is A - B. So:

A - B = (π/4) ln 2 + B - A.

Adding A + A - B - B = (π/4) ln 2.

2A - 2B = (π/4) ln 2.

Divide by 2: A - B = (π/8) ln 2.

Yes, that's correct. Therefore, the integral I is (π/8) ln 2. So the exact answer is (π/8) multiplied by ln 2? Wait, no, π/8 multiplied by ln 2. So (π ln 2)/8.

Wait, but let me check with a numerical approximation. Let's compute the integral numerically to see if it matches (π ln 2)/8.

Compute (π * ln 2)/8. Let's approximate:

π ≈ 3.1415926536

ln 2 ≈ 0.6931471806

Multiply them: 3.1415926536 * 0.6931471806 ≈ 2.1775860903

Divide by 8: 2.1775860903 / 8 ≈ 0.2721982613.

Wait, 2.1775860903 divided by 8 is approximately 0.2721982613.

But let's compute the integral numerically. Let's take x from 0 to π/4, compute ln(cot x -1) and integrate numerically. But integrating ln(cot x -1) from 0 to π/4. Let's see, at x approaching 0, cot x approaches infinity, so cot x -1 approaches infinity, ln(inf) is infinity. But the integral near 0 may be problematic. Wait, but let's check the behavior as x approaches 0:

cot x = cos x / sin x ≈ (1 - x²/2) / x ≈ 1/x - x/2. So cot x -1 ≈ (1/x - x/2) -1 ≈ (1 - x)/x - x/2. Wait, as x approaches 0, cot x -1 ~ 1/x -1. So ln(cot x -1) ~ ln(1/x -1) ~ ln(1/x) = -ln x. So the integral near 0 behaves like -ln x dx, which is integrable since ∫ -ln x dx from 0 to a is x - x ln x, which converges as x approaches 0.

Similarly, at x approaching π/4, cot x = 1, so cot x -1 =0, so ln(0) is -infinity. Wait, but cot(π/4) is 1, so cot x -1 approaches 0 as x approaches π/4 from below. So ln(cot x -1) approaches ln(0) which is -infinity. So the integrand tends to -infinity at x=π/4. Wait, but is the integral convergent there?

Let me check near x=π/4. Let t = π/4 - x, as t approaches 0+. Then cot(π/4 - t) -1 = [ (cos(π/4 - t) ) / sin(π/4 - t) ] -1. Let's expand cos(π/4 - t) = √2/2 (cos t + sin t) ≈ √2/2 (1 + t), and sin(π/4 - t) = √2/2 (cos t - sin t) ≈ √2/2 (1 - t). So cot(π/4 - t) ≈ (1 + t)/(1 - t). So cot(π/4 - t) -1 ≈ (1 + t)/(1 - t) -1 = [ (1 + t) - (1 - t) ] / (1 - t) = 2t / (1 - t) ≈ 2t. Therefore, ln(cot(π/4 - t) -1) ≈ ln(2t). So near t=0, the integrand behaves like ln(2t). The integral near t=0 is ∫ ln(2t) dt, which is t ln(2t) - t, which approaches 0 as t approaches 0. Therefore, the integral is convergent at both limits.

So the integral is convergent. Now, if the analytical result is (π ln 2)/8 ≈ 0.2721982613, let's check with approximate integration.

Alternatively, maybe I can use numerical integration method. Let's approximate the integral ∫₀^{π/4} ln(cot x -1) dx.

But since I don't compute it here, but according to the analytical steps, the result is (π ln 2)/8. Wait, but let me check the steps again.

Wait, when we did the substitution t = π/4 - x, and found that I = ∫₀^{π/4} [ln(2 sin t) - ln(cos t - sin t)] dt. Then, since the original I is also equal to ∫₀^{π/4} [ln(cos x - sin x) - ln(sin x)] dx, which is A - B. Then, by equating the two expressions for I, we arrived at I = (π/8) ln 2. So the exact answer is (π ln 2)/8.

But let me check with a different approach. Let's consider another substitution. Let’s set u = cot x -1. Then, du/dx = -csc²x. But this might not be helpful. Alternatively, set t = tan x. Then, when x=0, t=0; x=π/4, t=1. Then, cot x = 1/t, so cot x -1 = (1 - t)/t. So ln(cot x -1) = ln((1 - t)/t) = ln(1 - t) - ln t. Also, dx = dt/(1 + t²). So the integral becomes ∫₀¹ [ln(1 - t) - ln t] * (1/(1 + t²)) dt.

So I = ∫₀¹ [ln(1 - t) - ln t] / (1 + t²) dt.

This might be easier to handle. Let's split the integral into two parts:

I = ∫₀¹ ln(1 - t)/(1 + t²) dt - ∫₀¹ ln t / (1 + t²) dt.

Let’s denote the first integral as I1 and the second as I2.

I2 is a known integral. The integral of ln t / (1 + t²) dt from 0 to 1. Let me recall that ∫₀^∞ ln t / (1 + t²) dt = 0 by symmetry, but our integral is from 0 to 1. Let me compute I2.

Let’s substitute u = 1/t in I2. When t approaches 0, u approaches infinity. So:

I2 = ∫₀¹ ln t / (1 + t²) dt = ∫₁^∞ ln(1/u) / (1 + 1/u²) * (-du/u²) = ∫₁^∞ (-ln u) / (1 + 1/u²) * (du/u²) = ∫₁^∞ (-ln u) * u² / (1 + u²) * (du/u²) = ∫₁^∞ (-ln u) / (1 + u²) du.

But this is equal to -∫₁^∞ ln u / (1 + u²) du. Let’s change variable back to t = u, so I2 = -∫₁^∞ ln t / (1 + t²) dt. But if we add the original I2 and this expression:

I2 = -∫₁^∞ ln t / (1 + t²) dt.

But the original I2 is ∫₀¹ ln t / (1 + t²) dt. So, if we consider the integral from 0 to ∞, it's I2 + ∫₁^∞ ln t / (1 + t²) dt = ∫₀^∞ ln t / (1 + t²) dt = 0. Therefore, I2 + (-I2) = 0 => I2 - I2 = 0. Wait, that doesn't help. Alternatively, since the integral from 0 to ∞ is 0, then I2 = -∫₁^∞ ln t / (1 + t²) dt. Therefore, I2 = - ( - I2 ), which implies I2 = I2. Not helpful.

Alternatively, perhaps use series expansion. Let's expand 1/(1 + t²) as a power series. For |t| < 1, 1/(1 + t²) = Σ_{n=0}^∞ (-1)^n t^{2n}. So I2 = ∫₀¹ ln t Σ_{n=0}^∞ (-1)^n t^{2n} dt = Σ_{n=0}^∞ (-1)^n ∫₀¹ t^{2n} ln t dt.

Integrate term by term. The integral of t^{2n} ln t dt from 0 to 1. Let’s use substitution: let u = ln t, dv = t^{2n} dt. Then du = (1/t) dt, v = t^{2n +1}/(2n +1). Integration by parts gives:

uv|₀¹ - ∫ v du = [t^{2n +1}/(2n +1) ln t]₀¹ - ∫ t^{2n +1/(2n +1)} * (1/t) dt.

The first term: at t=1, it's 0. At t=0, t^{2n +1} ln t approaches 0 because t^{2n +1} approaches 0 and ln t approaches -infty, but the product tends to 0. The second term is -1/(2n +1) ∫ t^{2n} dt = -1/(2n +1) * [t^{2n +1}/(2n +1)] from 0 to1 = -1/(2n +1)^2.

Therefore, ∫₀¹ t^{2n} ln t dt = -1/(2n +1)^2.

Therefore, I2 = Σ_{n=0}^∞ (-1)^n * (-1)/(2n +1)^2 = Σ_{n=0}^∞ (-1)^{n+1}/(2n +1)^2.

This series is known. It's related to the Dirichlet beta function. Specifically, β(2) = Σ_{n=0}^∞ (-1)^n/(2n +1)^2. Therefore, I2 = -β(2).

The value of β(2) is known to be Catalan's constant G ≈ 0.9159655942. Wait, but Catalan's constant is Σ_{n=0}^∞ (-1)^n/(2n +1)^2 = β(2). So I2 = -G.

But wait, according to the calculation, I2 = Σ_{n=0}^∞ (-1)^{n+1}/(2n +1)^2 = - Σ_{n=0}^∞ (-1)^n/(2n +1)^2 = -β(2) = -G.

So I2 = -Catalan's constant.

Now, let's compute I1 = ∫₀¹ ln(1 - t)/(1 + t²) dt.

Again, perhaps expand 1/(1 + t²) as a power series. For t in [0,1), 1/(1 + t²) = Σ_{n=0}^∞ (-1)^n t^{2n}.

So I1 = ∫₀¹ ln(1 - t) Σ_{n=0}^∞ (-1)^n t^{2n} dt = Σ_{n=0}^∞ (-1)^n ∫₀¹ t^{2n} ln(1 - t) dt.

Let’s compute the integral ∫₀¹ t^{2n} ln(1 - t) dt. Let’s use integration by parts. Let u = ln(1 - t), dv = t^{2n} dt. Then du = -1/(1 - t) dt, v = t^{2n +1}/(2n +1).

So uv|₀¹ - ∫ v du = [t^{2n +1}/(2n +1) ln(1 - t)]₀¹ - ∫ t^{2n +1}/(2n +1) * (-1)/(1 - t) dt.

At t=1, ln(1 - t) approaches -infty, but t^{2n +1} approaches 1, so the first term is 0 - 0 = 0. At t=0, it's 0. So the integral becomes 1/(2n +1) ∫₀¹ t^{2n +1}/(1 - t) dt.

But ∫₀¹ t^{2n +1}/(1 - t) dt = ∫₀¹ t^{2n +1} Σ_{k=0}^∞ t^k dt = Σ_{k=0}^∞ ∫₀¹ t^{2n +1 +k} dt = Σ_{k=0}^∞ 1/(2n +k +2).

Therefore, ∫₀¹ t^{2n} ln(1 - t) dt = 1/(2n +1) Σ_{k=0}^∞ 1/(2n +k +2).

Let’s change index m = k + 2n +2, but not sure. Alternatively, note that Σ_{k=0}^∞ 1/(2n +k +2) = Σ_{m=2n +2}^∞ 1/m = ψ(2n +2) + γ, where ψ is the digamma function and γ is Euler-Mascheroni constant. But this might not be helpful.

Alternatively, recognize that Σ_{k=0}^∞ 1/(2n +k +2) = Σ_{m=0}^∞ 1/(m + 2n +2) = ζ(1) - Σ_{m=0}^{2n +1} 1/(m +1). But ζ(1) diverges, so this approach isn't helpful.

Alternatively, perhaps express the sum as an integral. Σ_{k=0}^∞ 1/(2n +k +2) = Σ_{k=0}^∞ ∫₀¹ t^{2n +k +1} dt = ∫₀¹ t^{2n +1} Σ_{k=0}^∞ t^k dt = ∫₀¹ t^{2n +1}/(1 - t) dt. But this brings us back to the original integral. So this approach isn't helpful.

Alternatively, perhaps use the integral representation of the digamma function. But this seems complicated.

Alternatively, note that ∫₀¹ t^{2n} ln(1 - t) dt = - Σ_{k=1}^∞ ∫₀¹ t^{2n +k}/k dt = - Σ_{k=1}^∞ 1/(k(2n +k +1)).

But this series might not be easily summable.

Alternatively, perhaps use the expansion of ln(1 - t) as -Σ_{m=1}^∞ t^m/m. Then,

I1 = ∫₀¹ ln(1 - t)/(1 + t²) dt = -∫₀¹ Σ_{m=1}^∞ t^m/m * Σ_{n=0}^∞ (-1)^n t^{2n} dt.

Multiply the two series:

= -Σ_{m=1}^∞ Σ_{n=0}^∞ (-1)^n/m ∫₀¹ t^{m + 2n} dt.

= -Σ_{m=1}^∞ Σ_{n=0}^∞ (-1)^n/(m (m + 2n +1)).

This double series might be challenging to evaluate, but perhaps we can interchange the order of summation. Let’s set k = m + 2n. For fixed k, m can range from 1 to k, and n = (k - m)/2. But since n must be an integer, k - m must be even, so m must have the same parity as k. This seems complicated.

Alternatively, perhaps use substitution in I1. Let’s set u = 1 - t. Then, when t=0, u=1; t=1, u=0. So I1 = ∫₁⁰ ln u / (1 + (1 - u)^2) (-du) = ∫₀¹ ln u / (1 + (1 - u)^2) du.

Expand the denominator: 1 + (1 - u)^2 = 1 + 1 - 2u + u² = 2 - 2u + u². Not sure if this helps.

Alternatively, perhaps use substitution u = tan θ. Let’s set t = tan θ, but not sure.

Alternatively, consider that I1 and I2 are related. Let’s see:

I = I1 - I2 = [∫₀¹ ln(1 - t)/(1 + t²) dt] - [∫₀¹ ln t / (1 + t²) dt].

But I1 can be expressed as ∫₀¹ ln(1 - t)/(1 + t²) dt. Let’s consider substituting t = (1 - u)/(1 + u). This is a Möbius substitution that sometimes helps in integrals involving 1 + t². Let’s try:

Let u = (1 - t)/(1 + t). Then, t = (1 - u)/(1 + u), dt = -2 du/(1 + u)^2.

When t=0, u=1; t=1, u=0. So the integral becomes:

I1 = ∫₁⁰ ln(1 - (1 - u)/(1 + u)) / (1 + [(1 - u)/(1 + u)]²) * (-2 du/(1 + u)^2).

Simplify the expression inside the logarithm:

1 - (1 - u)/(1 + u) = [ (1 + u) - (1 - u) ] / (1 + u) = (2u)/(1 + u).

The denominator:

1 + [(1 - u)^2/(1 + u)^2] = [ (1 + u)^2 + (1 - u)^2 ] / (1 + u)^2 = [1 + 2u + u² + 1 - 2u + u²]/(1 + u)^2 = [2 + 2u²]/(1 + u)^2) = 2(1 + u²)/(1 + u)^2.

So the integral becomes:

I1 = ∫₀¹ ln(2u/(1 + u)) / [2(1 + u²)/(1 + u)^2] * 2 du/(1 + u)^2.

Simplify step by step:

First, the numerator of the fraction inside the integral is ln(2u/(1 + u)).

The denominator is 2(1 + u²)/(1 + u)^2.

So the entire fraction is [ln(2u/(1 + u))] / [2(1 + u²)/(1 + u)^2] = [ln(2u) - ln(1 + u)] * (1 + u)^2 / [2(1 + u²)].

Then, multiply by the Jacobian 2/(1 + u)^2:

So the integrand becomes [ln(2u) - ln(1 + u)] * (1 + u)^2 / [2(1 + u²)] * 2/(1 + u)^2) = [ln(2u) - ln(1 + u)] / (1 + u²).

Therefore, I1 = ∫₀¹ [ln(2u) - ln(1 + u)] / (1 + u²) du.

Split this into two integrals:

I1 = ∫₀¹ ln(2u)/(1 + u²) du - ∫₀¹ ln(1 + u)/(1 + u²) du.

The first integral is ln 2 ∫₀¹ 1/(1 + u²) du + ∫₀¹ ln u/(1 + u²) du.

The integral of 1/(1 + u²) from 0 to1 is π/4. The second integral is I2. So:

First part: ln 2 * π/4 + I2.

Second part: ∫₀¹ ln(1 + u)/(1 + u²) du. Let’s denote this as I3.

So I1 = (π/4 ln 2 + I2) - I3.

But I1 = ∫₀¹ ln(1 - t)/(1 + t²) dt, which we transformed into this expression. Therefore:

I1 = (π/4 ln 2 + I2) - I3.

But we also have I = I1 - I2 = (π/4 ln 2 + I2 - I3) - I2 = π/4 ln 2 - I3.

But we need to find I3 = ∫₀¹ ln(1 + u)/(1 + u²) du.

Let’s compute I3. Let’s use substitution u = tan θ. Then, du = sec²θ dθ, 1 + u² = sec²θ. When u=0, θ=0; u=1, θ=π/4.

So I3 = ∫₀^{π/4} ln(1 + tan θ) dθ.

This integral is known. Let’s recall that ∫₀^{π/4} ln(1 + tan θ) dθ = (π/8) ln 2. This is a standard integral. Let me verify:

Let’s use substitution φ = π/4 - θ. Then, when θ=0, φ=π/4; θ=π/4, φ=0.

I3 = ∫_{π/4}^0 ln(1 + tan(π/4 - φ)) (-dφ) = ∫₀^{π/4} ln(1 + tan(π/4 - φ)) dφ.

Now, tan(π/4 - φ) = (1 - tan φ)/(1 + tan φ). So:

I3 = ∫₀^{π/4} ln(1 + (1 - tan φ)/(1 + tan φ)) dφ.

Simplify the logarithm:

1 + (1 - tan φ)/(1 + tan φ) = [ (1 + tan φ) + (1 - tan φ) ] / (1 + tan φ) = 2 / (1 + tan φ).

Therefore, ln(2 / (1 + tan φ)) = ln 2 - ln(1 + tan φ).

So I3 = ∫₀^{π/4} [ln 2 - ln(1 + tan φ)] dφ = ln 2 * (π/4) - ∫₀^{π/4} ln(1 + tan φ) dφ.

But this integral is I3 itself. So:

I3 = (π/4) ln 2 - I3.

Bring I3 to the left:

2I3 = (π/4) ln 2.

Therefore, I3 = (π/8) ln 2.

So going back to I = π/4 ln 2 - I3 = π/4 ln 2 - (π/8) ln 2 = (2π/8 - π/8) ln 2 = (π/8) ln 2.

Therefore, the integral I is indeed (π/8) ln 2. So the exact answer is (π ln 2)/8.

Now, the numerical approximation. As calculated earlier, π ≈ 3.1415926536, ln 2 ≈ 0.6931471806.

Multiply them: 3.1415926536 * 0.6931471806 ≈ 2.1775860903.

Divide by 8: 2.1775860903 / 8 ≈ 0.2721982613.

Rounded to 10 decimal places, this is approximately 0.2721982613.

Therefore, the final answer is {"answer": "\\dfrac{\\pi \\ln 2}{8}", "numerical_answer": "0.2721982613"}.
</think>

{"answer": "\\dfrac{\\pi \\ln 2}{8}", "numerical_answer": "0.2721982613"}