Let's solve the integral:
\[
I = \int_0^1 \sqrt[4]{\frac{1}{x} - 1} \, dx
\]

### Step 1: Substitution

Let us use the substitution:
\( x = \sin^2 \theta \), so as \( x \) goes from 0 to 1, \( \theta \) goes from 0 to \( \frac{\pi}{2} \).

Now,
\[
dx = 2\sin\theta\cos\theta\ d\theta = \sin(2\theta)\ d\theta
\]

The integrand:
\[
\frac{1}{x}-1 = \frac{1}{\sin^2\theta} - 1 = \frac{1 - \sin^2\theta}{\sin^2\theta} = \frac{\cos^2\theta}{\sin^2\theta} = \cot^2\theta
\]
So,
\[
\sqrt[4]{\frac{1}{x} - 1}
= \sqrt[4]{\cot^2\theta}
= (\cot^2\theta)^{1/4}
= (\cot\theta)^{1/2}
= (\tan\theta)^{-1/2}
\]

Now, in terms of \( \theta \):

\[
I = \int_{x=0}^{x=1} \sqrt[4]{\frac{1}{x} - 1} dx = \int_{\theta=0}^{\theta=\frac{\pi}{2}} (\tan\theta)^{-1/2} \cdot 2\sin\theta\cos\theta\, d\theta
\]

But \((\tan\theta)^{-1/2} = (\cot\theta)^{1/2} = \frac{\cos^{1/2}\theta}{\sin^{1/2}\theta}\).

Also, \(2\sin\theta\cos\theta = \sin(2\theta)\).

So,

\[
I = \int_0^{\frac{\pi}{2}} \left(\frac{\cos^{1/2}\theta}{\sin^{1/2}\theta}\right)\ \sin(2\theta)\ d\theta
\]

Letâ€™s write this more clearly:

\[
I = \int_0^{\frac{\pi}{2}} \frac{\cos^{1/2}\theta}{\sin^{1/2}\theta} \cdot \sin(2\theta)\ d\theta
\]
Recall that:
\(\sin(2\theta) = 2\sin\theta\cos\theta\)

So:

\[
I = \int_0^{\frac{\pi}{2}} \frac{\cos^{1/2}\theta}{\sin^{1/2}\theta} \cdot 2\sin\theta\cos\theta\ d\theta
\]
\[
= 2\int_0^{\frac{\pi}{2}} \frac{\cos^{1/2}\theta}{\sin^{1/2}\theta} \sin\theta\cos\theta\ d\theta
\]

The powers combine:

\[
\frac{\cos^{1/2}\theta}{\sin^{1/2}\theta} \cdot \sin\theta \cos\theta 
= \sin^{1-1/2}\theta \cdot \cos^{1+1/2}\theta
= \sin^{1/2}\theta \cdot \cos^{3/2}\theta 
\]

So:

\[
I = 2\int_0^{\frac{\pi}{2}} \sin^{1/2}\theta \cos^{3/2}\theta \ d\theta
\]

### Step 2: Beta Function Representation

Recall:
\[
\int_0^{\frac{\pi}{2}} \sin^{a-1}\theta \cos^{b-1}\theta\ d\theta = \frac{1}{2} \mathrm{B}\left(\frac{a}{2}, \frac{b}{2}\right)
\]
where \(\mathrm{B}(p,q)\) is the Beta function.

For us:
- \(\sin^{1/2}\theta = \sin^{(3/2 - 1)}\theta\) (\(a = 3/2\))
- \(\cos^{3/2}\theta = \cos^{(5/2 - 1)}\theta\) (\(b = 5/2\))

So,
\[
I = 2\cdot \int_0^{\frac{\pi}{2}} \sin^{1/2}\theta\ \cos^{3/2}\theta\ d\theta \\
= 2 \cdot \int_0^{\frac{\pi}{2}} \sin^{(3/2) - 1}\theta\ \cos^{(5/2) - 1}\theta\ d\theta \\
= 2 \cdot \frac{1}{2} \mathrm{B}\left(\frac{3/2}{2}, \frac{5/2}{2}\right) \\
= \mathrm{B}\left(\frac{3}{4}, \frac{5}{4}\right)
\]

So,

\[
I = \boxed{\mathrm{B}\left(\frac{3}{4}, \frac{5}{4}\right)}
\]

Expressing the Beta function in terms of Gamma functions:

\[
\mathrm{B}\left(\frac{3}{4}, \frac{5}{4}\right) = \frac{\Gamma\left(\frac{3}{4}\right)\Gamma\left(\frac{5}{4}\right)}{\Gamma(2)}
\]
but \(\Gamma(2) = 1\), so

\[
I = \Gamma\left(\frac{3}{4}\right)\Gamma\left(\frac{5}{4}\right)
\]

Now, recall that \(\Gamma(z+1) = z\Gamma(z)\), so
\[
\Gamma\left(\frac{5}{4}\right) = \frac{1}{4}\Gamma\left(\frac{1}{4}\right)
\]
So,
\[
I = \Gamma\left(\frac{3}{4}\right) \cdot \frac{1}{4}\Gamma\left(\frac{1}{4}\right)
\]

Thus, another possible closed form is:
\[
I = \frac{1}{4}\Gamma\left(\frac{1}{4}\right)\Gamma\left(\frac{3}{4}\right)
\]

### Step 3: Numerical Evaluation

Now let's compute the numerical value.

\[
\Gamma\left(\frac{1}{4}\right) \approx 3.6256099082
\]
\[
\Gamma\left(\frac{3}{4}\right) \approx 1.2254167025
\]

Thus,
\[
I \approx \frac{1}{4} \times 3.6256099082 \times 1.2254167025 \\
= \frac{1}{4} \times 4.4428829381 \\
= 1.1107207345
\]

### Step 4: Final JSON Output

```json
{"answer": "\\Gamma\\left(\\frac{3}{4}\\right)\\Gamma\\left(\\frac{5}{4}\\right)", "numerical_answer": "1.1107207345"}
```