# Definite Integral Evaluation: $\int_{0}^{2}x^{-1/2}(2-x)^{1/2}[1-0.5x(2-x)]^{1/2}dx$

I'll solve this definite integral analytically, following all the required steps.

## Step 1: Examine the integrand and consider substitution

Let's work with the integrand:
$$x^{-1/2}(2-x)^{1/2}[1-0.5x(2-x)]^{1/2}$$

First, I notice that the limits are from 0 to 2, and the expression involves $x$ and $(2-x)$ in a somewhat symmetric way. This suggests a substitution that highlights this symmetry.

Let's substitute $x = 2\sin^2\theta$, which implies $2-x = 2(1-\sin^2\theta) = 2\cos^2\theta$.

## Step 2: Apply the substitution

When $x = 2\sin^2\theta$:
- $dx = 4\sin\theta\cos\theta\,d\theta$
- $x^{-1/2} = (2\sin^2\theta)^{-1/2} = \frac{1}{\sqrt{2}\sin\theta}$
- $(2-x)^{1/2} = (2\cos^2\theta)^{1/2} = \sqrt{2}\cos\theta$
- $x(2-x) = 2\sin^2\theta \cdot 2\cos^2\theta = 4\sin^2\theta\cos^2\theta$
- $[1-0.5x(2-x)]^{1/2} = [1-0.5 \cdot 4\sin^2\theta\cos^2\theta]^{1/2} = [1-2\sin^2\theta\cos^2\theta]^{1/2}$

The term $\sin^2\theta\cos^2\theta$ can be rewritten as $\frac{1}{4}\sin^2(2\theta)$, so:
- $[1-2\sin^2\theta\cos^2\theta]^{1/2} = [1-\frac{1}{2}\sin^2(2\theta)]^{1/2}$

## Step 3: Transform the integral with the new substitution

Substituting all these expressions:

$$\int_{0}^{2}x^{-1/2}(2-x)^{1/2}[1-0.5x(2-x)]^{1/2}dx$$

$$= \int_{\theta=0}^{\theta=\pi/2} \frac{1}{\sqrt{2}\sin\theta} \cdot \sqrt{2}\cos\theta \cdot [1-\frac{1}{2}\sin^2(2\theta)]^{1/2} \cdot 4\sin\theta\cos\theta\,d\theta$$

$$= 4 \int_{0}^{\pi/2} \cos^2\theta \cdot [1-\frac{1}{2}\sin^2(2\theta)]^{1/2} \,d\theta$$

## Step 4: Further simplification

Using the identity $\cos^2\theta = \frac{1+\cos(2\theta)}{2}$:

$$= 4 \int_{0}^{\pi/2} \frac{1+\cos(2\theta)}{2} \cdot [1-\frac{1}{2}\sin^2(2\theta)]^{1/2} \,d\theta$$

$$= 2 \int_{0}^{\pi/2} (1+\cos(2\theta)) \cdot [1-\frac{1}{2}\sin^2(2\theta)]^{1/2} \,d\theta$$

Let's introduce another substitution: $\phi = 2\theta$, which means $d\theta = \frac{d\phi}{2}$.

When $\theta = 0$, $\phi = 0$, and when $\theta = \pi/2$, $\phi = \pi$.

$$= 2 \int_{0}^{\pi} (1+\cos\phi) \cdot [1-\frac{1}{2}\sin^2\phi]^{1/2} \cdot \frac{1}{2} \,d\phi$$

$$= \int_{0}^{\pi} (1+\cos\phi) \cdot [1-\frac{1}{2}\sin^2\phi]^{1/2} \,d\phi$$

## Step 5: Recognize a standard form

The expression $[1-\frac{1}{2}\sin^2\phi]^{1/2}$ can be rewritten as $[1-k^2\sin^2\phi]^{1/2}$ with $k^2 = \frac{1}{2}$ or $k = \frac{1}{\sqrt{2}}$.

This is related to the complete elliptic integral of the second kind, denoted as $E(k)$.

The standard form is:
$$E(k) = \int_{0}^{\pi/2} [1-k^2\sin^2\phi]^{1/2} \,d\phi$$

But our integral is slightly different. We have:
$$\int_{0}^{\pi} (1+\cos\phi) \cdot [1-\frac{1}{2}\sin^2\phi]^{1/2} \,d\phi$$

Due to symmetry, we can write:
$$\int_{0}^{\pi} (1+\cos\phi) \cdot [1-\frac{1}{2}\sin^2\phi]^{1/2} \,d\phi = 2\int_{0}^{\pi/2} (1+\cos\phi) \cdot [1-\frac{1}{2}\sin^2\phi]^{1/2} \,d\phi$$

## Step 6: Evaluate the integral in terms of complete elliptic integrals

The integral can be expressed in terms of complete elliptic integrals:

$$2\int_{0}^{\pi/2} [1-\frac{1}{2}\sin^2\phi]^{1/2} \,d\phi + 2\int_{0}^{\pi/2} \cos\phi \cdot [1-\frac{1}{2}\sin^2\phi]^{1/2} \,d\phi$$

The first part is $2E(\frac{1}{\sqrt{2}})$.

For the second part, we can use the substitution $u = \sin\phi$, which gives $du = \cos\phi\,d\phi$:

$$2\int_{0}^{\pi/2} \cos\phi \cdot [1-\frac{1}{2}\sin^2\phi]^{1/2} \,d\phi = 2\int_{0}^{1} [1-\frac{1}{2}u^2]^{1/2} \,du$$

This is a straightforward integral. Let $v = \frac{1}{2}u^2$, which gives $dv = u\,du$, or $du = \frac{dv}{u} = \frac{dv}{\sqrt{2v}}$:

$$2\int_{0}^{1} [1-\frac{1}{2}u^2]^{1/2} \,du = 2\int_{0}^{1/2} [1-v]^{1/2} \cdot \frac{1}{\sqrt{2v}} \,dv$$

$$= \frac{2}{\sqrt{2}}\int_{0}^{1/2} \frac{[1-v]^{1/2}}{\sqrt{v}} \,dv$$

This is a beta function. Specifically, $B(\frac{1}{2}, \frac{3}{2}) = \int_{0}^{1} v^{-1/2}(1-v)^{1/2} \,dv = \frac{\Gamma(1/2)\Gamma(3/2)}{\Gamma(2)} = \frac{\sqrt{\pi} \cdot \frac{\sqrt{\pi}}{2}}{1} = \frac{\pi}{2}$.

So, we have:
$$\frac{2}{\sqrt{2}}\int_{0}^{1/2} \frac{[1-v]^{1/2}}{\sqrt{v}} \,dv = \frac{2}{\sqrt{2}} \cdot \frac{\pi}{2} \cdot \frac{1}{2^{1/2}} = \frac{\pi}{2}$$

## Step 7: Final calculation

The definite integral equals:
$$2E(\frac{1}{\sqrt{2}}) + \frac{\pi}{2}$$

Using the known value of $E(\frac{1}{\sqrt{2}}) = \frac{\Gamma(1/2)\Gamma(1)}{\Gamma(3/2)} \cdot \frac{1}{2} \cdot \pi^{1/2} = \frac{\sqrt{\pi} \cdot 1}{\frac{\sqrt{\pi}}{2}} \cdot \frac{1}{2} \cdot \sqrt{\pi} = \frac{\pi}{2}$

Therefore:
$$2E(\frac{1}{\sqrt{2}}) + \frac{\pi}{2} = 2 \cdot \frac{\pi}{2} + \frac{\pi}{2} = \pi + \frac{\pi}{2} = \frac{3\pi}{2}$$

## Step 8: Numerical approximation

The exact answer is $\frac{3\pi}{2}$.
Numerically, $\frac{3\pi}{2} = 4.7123889803846898576939650749193...$

Rounded to 10 decimal places: $4.7123889804$

{"answer": "\\frac{3\\pi}{2}", "numerical_answer": "4.7123889804"}