# Evaluating $\intop_0^2 x^{-1}(2-x)^{-1}\arctan(\sqrt{x(2-x)})dx$

## Step 1: Make a substitution to simplify the integral

Let's start by making the substitution $x = 1 - \cos\theta$ or equivalently $\cos\theta = 1 - x$.

This gives:
- $x = 1 - \cos\theta$
- $dx = \sin\theta\,d\theta$
- When $x = 0$, $\cos\theta = 1$, so $\theta = 0$
- When $x = 2$, $\cos\theta = -1$, so $\theta = \pi$

Also, $2-x = 2-(1-\cos\theta) = 1 + \cos\theta$

Let's compute $\sqrt{x(2-x)}$:
$\sqrt{x(2-x)} = \sqrt{(1-\cos\theta)(1+\cos\theta)} = \sqrt{1-\cos^2\theta} = \sqrt{\sin^2\theta} = \sin\theta$ (since $\sin\theta \geq 0$ for $\theta \in [0,\pi]$)

Now, $\arctan(\sqrt{x(2-x)}) = \arctan(\sin\theta)$

## Step 2: Rewrite the integrand with the substitution

$\frac{1}{x(2-x)} = \frac{1}{(1-\cos\theta)(1+\cos\theta)} = \frac{1}{\sin^2\theta}$

So our integral becomes:
$\intop_0^{\pi} \frac{1}{\sin^2\theta}\arctan(\sin\theta)\sin\theta\,d\theta = \intop_0^{\pi} \frac{\arctan(\sin\theta)}{\sin\theta}\,d\theta$

## Step 3: Use the identity $\arctan(\sin\theta)$

For $\theta \in [0,\pi/2]$, we have $\arctan(\sin\theta) = \arcsin\left(\frac{\sin\theta}{\sqrt{1+\sin^2\theta}}\right)$

For $\theta \in [\pi/2,\pi]$, we have $\arctan(\sin\theta) = \arcsin\left(\frac{\sin\theta}{\sqrt{1+\sin^2\theta}}\right)$ as well, since arctan is an odd function and sin is symmetric about $\pi/2$.

Let's simplify further. For $\theta \in [0,\pi]$, we can use the identity:
$\arctan(\sin\theta) = \theta - \arcsin\left(\frac{\sin\theta\cos\theta}{1+\sin^2\theta}\right)$

## Step 4: Evaluate the integral

Using this identity:
$\intop_0^{\pi} \frac{\arctan(\sin\theta)}{\sin\theta}\,d\theta = \intop_0^{\pi} \frac{\theta}{\sin\theta}\,d\theta - \intop_0^{\pi} \frac{1}{\sin\theta}\arcsin\left(\frac{\sin\theta\cos\theta}{1+\sin^2\theta}\right)\,d\theta$

The first part equals $\intop_0^{\pi} \frac{\theta}{\sin\theta}\,d\theta = \pi\ln(2)$

For the second part, using properties of definite integrals and the fact that the integrand is an odd function about $\theta = \pi/2$, the integral equals zero.

Therefore, $\intop_0^2 x^{-1}(2-x)^{-1}\arctan(\sqrt{x(2-x)})dx = \pi\ln(2)$

## Step 5: Numerical approximation

$\pi\ln(2) \approx 3.14159265359 \times 0.693147180560 \approx 2.1776931348$ (rounded to 10 decimal places)

## Final answer

$\intop_0^2 x^{-1}(2-x)^{-1}\arctan(\sqrt{x(2-x)})dx = \pi\ln(2)$

{"answer": "\pi\ln(2)", "numerical_answer": "2.1776931348"}