

To solve the definite integral \(\int\limits_0^{2} x^{1 - 3/2}(2 - x)^{1 - 1/2}[1 - 0.5x(2 - x)]^{-1} \, dx\), we proceed as follows:

### Step 1: Simplify the integrand
First, simplify the exponents and the denominator:
- \(x^{1 - 3/2} = x^{-1/2}\)
- \((2 - x)^{1 - 1/2} = (2 - x)^{1/2}\)
- The denominator \(1 - 0.5x(2 - x) = 1 - x + \frac{x^2}{2} = \frac{(x - 1)^2 + 1}{2}\).

Thus, the integrand becomes:
\[
x^{-1/2}(2 - x)^{1/2} \cdot \frac{2}{(x - 1)^2 + 1}
\]

### Step 2: Substitution \(u = x - 1\)
Let \(u = x - 1\), so \(x = u + 1\) and \(dx = du\). The limits change from \(x = 0\) to \(u = -1\) and \(x = 2\) to \(u = 1\). The integrand transforms to:
\[
(u + 1)^{-1/2}(1 - u)^{1/2} \cdot \frac{2}{u^2 + 1}
\]

### Step 3: Split the integral and simplify
The integral becomes \(2 \int_{-1}^1 \frac{(u + 1)^{-1/2}(1 - u)^{1/2}}{u^2 + 1} \, du\). Splitting the integral into \([-1, 0]\) and \([0, 1]\), and substituting \(u = -v\) for the \([-1, 0]\) interval, we combine the results to find:
\[
2 \left[ \int_0^1 \frac{(1 + t)^{1/2}(1 - t)^{-1/2} + (1 + t)^{-1/2}(1 - t)^{1/2}}{t^2 + 1} \, dt \right]
\]

### Step 4: Further simplification
Factor out \((1 + t)^{-1/2}(1 - t)^{-1/2}\) from the numerator, leading to:
\[
4 \int_0^1 \frac{1}{\sqrt{1 - t^2}(t^2 + 1)} \, dt
\]

### Step 5: Trigonometric substitution \(t = \sin\theta\)
Let \(t = \sin\theta\), so \(dt = \cos\theta \, d\theta\) and \(\sqrt{1 - t^2} = \cos\theta\). The integral simplifies to:
\[
4 \int_0^{\pi/2} \frac{1}{1 + \sin^2\theta} \, d\theta
\]

### Step 6: Evaluate the trigonometric integral
Using \(u = \tan\theta\), the integral becomes:
\[
4 \cdot \frac{\pi}{2\sqrt{2}} = \pi\sqrt{2}
\]

### Numerical Approximation
The numerical value of \(\pi\sqrt{2}\) is approximately \(4.4428829081\) (rounded to 10 decimal places).

{"answer": "\(\pi\sqrt{2}\)", "numerical_answer": "4.4428829081"}