We wish to evaluate

  I = ∫₀² [arctan(x)]⁄[x √(4 – x²)] dx.

Step 1. Substitution

Let x = 2 sinθ. Then
  dx = 2 cosθ dθ  and  √(4 – x²) = √(4 – 4 sin²θ) = 2 cosθ.
The limits become:
  x = 0 → sinθ = 0, so θ = 0,
  x = 2 → sinθ = 1, so θ = π/2.

Substitute into I:

  I = ∫₀^(π/2) [arctan(2 sinθ)]⁄[(2 sinθ)(2 cosθ)] · (2 cosθ dθ)
     = ∫₀^(π/2) arctan(2 sinθ)⁄(4 sinθ cosθ) · 2 cosθ dθ
     = (1/2) ∫₀^(π/2) [arctan(2 sinθ)]⁄(sinθ) dθ.

Thus, we have

  I = (1/2) J   where  J = ∫₀^(π/2) [arctan(2 sinθ)]⁄(sinθ) dθ.

Step 2. Differentiation under the Integral Sign

To handle J, define a function depending on a parameter a:

  I(a) = ∫₀^(π/2) [arctan(a sinθ)]⁄(sinθ) dθ.

Notice that our desired J is I(2).

Differentiate I(a) with respect to a. Interchange differentiation and integration:
  dI/da = ∫₀^(π/2) d/da { arctan(a sinθ) }⁄(sinθ) dθ.
Since d/da arctan(a sinθ) = sinθ/(1 + a² sin²θ), we get
  dI/da = ∫₀^(π/2) [sinθ/(1 + a² sin²θ)]⁄(sinθ) dθ
      = ∫₀^(π/2) 1/(1 + a² sin²θ) dθ.

A standard integral formula tells us
  ∫₀^(π/2) dθ/(1 + a² sin²θ) = π/(2√(1 + a²)).

Thus,
  dI/da = π/(2√(1 + a²)).

Integrate with respect to a:
  I(a) = ∫₀^a [π/(2√(1 + t²))] dt = (π/2) sinh⁻¹(a),
since sinh⁻¹(a) = ∫₀^a 1/√(1 + t²) dt.

The constant of integration is zero because I(0) = 0 (note that arctan(0) = 0).

Hence,
  I(a) = (π/2) sinh⁻¹(a) = (π/2) ln[a + √(a² + 1)].

Step 3. Obtain the Answer

Returning to our function, recall that we needed I(2). Thus,

  J = I(2) = (π/2) ln(2 + √(2² + 1))
      = (π/2) ln(2 + √5).

Then the original integral is

  I = (1/2) J = (1/2) · (π/2) ln(2 + √5) = (π/4) ln(2 + √5).

Step 4. Numerical Approximation

We have:
  √5 ≈ 2.2360679775 ⇒ 2 + √5 ≈ 4.2360679775,
  ln(4.2360679775) ≈ 1.443635475,
  π/4 ≈ 0.7853981634.

Thus, the numerical value is approximately:

  (π/4) ln(2 + √5) ≈ 0.7853981634 × 1.443635475 ≈ 1.1339745960.

Final Answer in JSON format:

{"answer": "\\frac{\\pi}{4}\\ln(2+\\sqrt{5})", "numerical_answer": "1.1339745960"}