
To compute the definite integral \(\int_0^{\frac{\pi}{2}} x \ln(\sin x) \, dx\), we proceed as follows:

### Step 1: Series Expansion of \(\ln(\sin x)\)
The function \(\ln(\sin x)\) can be expressed as a Fourier series for \(0 < x < \pi\):
\[
\ln(\sin x) = -\ln 2 - \sum_{n=1}^{\infty} \frac{\cos(2nx)}{n}
\]

### Step 2: Substitute the Series into the Integral
Substituting this series into the integral, we get:
\[
\int_0^{\frac{\pi}{2}} x \ln(\sin x) \, dx = \int_0^{\frac{\pi}{2}} x \left( -\ln 2 - \sum_{n=1}^{\infty} \frac{\cos(2nx)}{n} \right) dx
\]
This splits into two terms:
\[
= -\ln 2 \int_0^{\frac{\pi}{2}} x \, dx - \sum_{n=1}^{\infty} \frac{1}{n} \int_0^{\frac{\pi}{2}} x \cos(2nx) \, dx
\]

### Step 3: Evaluate the First Integral
The first integral is straightforward:
\[
\int_0^{\frac{\pi}{2}} x \, dx = \left. \frac{x^2}{2} \right|_0^{\frac{\pi}{2}} = \frac{\pi^2}{8}
\]
Thus, the first term becomes:
\[
-\ln 2 \cdot \frac{\pi^2}{8}
\]

### Step 4: Evaluate the Series Term
For the series term, we compute \(\int_0^{\frac{\pi}{2}} x \cos(2nx) \, dx\) using integration by parts. Let \(u = x\) and \(dv = \cos(2nx) \, dx\). Then \(du = dx\) and \(v = \frac{\sin(2nx)}{2n}\). Applying integration by parts:
\[
\int x \cos(2nx) \, dx = \frac{x \sin(2nx)}{2n} + \frac{\cos(2nx)}{4n^2}
\]
Evaluating from \(0\) to \(\frac{\pi}{2}\):
\[
\left. \frac{x \sin(2nx)}{2n} + \frac{\cos(2nx)}{4n^2} \right|_0^{\frac{\pi}{2}} = \frac{\cos(n\pi)}{4n^2} - \frac{1}{4n^2} = \frac{(-1)^n - 1}{4n^2}
\]
(Note: \(\sin(n\pi) = 0\) and \(\cos(n\pi) = (-1)^n\).)

### Step 5: Simplify the Series
Substituting back, the series term becomes:
\[
- \sum_{n=1}^{\infty} \frac{1}{n} \cdot \frac{(-1)^n - 1}{4n^2} = - \frac{1}{4} \sum_{n=1}^{\infty} \frac{(-1)^n - 1}{n^3}
\]
For even \(n\), \((-1)^n - 1 = 0\). For odd \(n\), \((-1)^n - 1 = -2\). Thus, the series reduces to:
\[
- \frac{1}{4} \left( -2 \sum_{k=1}^{\infty} \frac{1}{(2k-1)^3} \right) = \frac{1}{2} \sum_{k=1}^{\infty} \frac{1}{(2k-1)^3}
\]
Using \(\sum_{k=1}^{\infty} \frac{1}{(2k-1)^3} = \left(1 - \frac{1}{2^3}\right) \zeta(3) = \frac{7}{8} \zeta(3)\), we get:
\[
\frac{1}{2} \cdot \frac{7}{8} \zeta(3) = \frac{7}{16} \zeta(3)
\]

### Step 6: Combine Terms
Combining the results, the integral is:
\[
\int_0^{\frac{\pi}{2}} x \ln(\sin x) \, dx = \frac{7}{16} \zeta(3) - \frac{\pi^2}{8} \ln 2
\]

### Numerical Approximation
Using \(\zeta(3) \approx 1.202056903159594\), \(\pi^2 \approx 9.8696044\), and \(\ln 2 \approx 0.69314718056\):
\[
\frac{7}{16} \zeta(3) \approx 0.5258998951, \quad \frac{\pi^2}{8} \ln 2 \approx 0.855893304
\]
Thus, the numerical approximation is:
\[
0.5258998951 - 0.855893304 \approx -0.3299934089
\]

{"answer": "\\frac{7}{16}\\zeta(3) - \\frac{\\pi^2}{8}\\ln 2", "numerical_answer": "-0.3299934089"}