We will show that the integral

  I = ∫₀² x^(1/2) (2–x)^(1/2) cos(√(x(2–x))) dx

can be transformed into an expression in terms of Bessel functions. One acceptable answer is

  I = (π/2)[J₀(1) – J₂(1)].

In what follows we describe one route to this result.

Step 1. A change of variable to center the interval

Let
  x = 1 + u  so that  2 – x = 1 – u.
Then as x runs from 0 to 2, u runs from –1 to 1. Also notice that
  √(x(2–x)) = √((1+u)(1–u)) = √(1 – u²)
and
  x^(1/2)(2–x)^(1/2) = √(1 – u²).
Since dx = du the integral becomes
  I = ∫₋₁¹ √(1 – u²) cos(√(1 – u²)) du.

Step 2. Changing to an angular variable

Now set
  u = sinθ,  so that  du = cosθ dθ  and  √(1 – u²) = cosθ.
When u = –1, θ = –π/2 and when u = 1, θ = π/2. Hence,
  I = ∫₋π/2^(π/2) cosθ · cos( cosθ ) · cosθ dθ
    = ∫₋π/2^(π/2) cos²θ · cos( cosθ ) dθ.
Because the integrand is even we can write
  I = 2∫₀^(π/2) cos²θ · cos( cosθ ) dθ.

Step 3. Expressing cos²θ in a convenient form

Recall that
  cos²θ = (1 + cos2θ)/2.
Thus,
  I = 2∫₀^(π/2) (1+cos2θ)/2 · cos(cosθ)dθ
    = ∫₀^(π/2) [1 + cos2θ] cos(cosθ) dθ.
That is, the integral splits into
  I = I₁ + I₂,  with
  I₁ = ∫₀^(π/2) cos(cosθ)dθ  and  I₂ = ∫₀^(π/2) cos2θ · cos(cosθ)dθ.

Step 4. Extending the integration range

One may show (using the symmetry of the integrands) that the integrals over [0, π/2] are exactly one‐half of the integrals over [0, π]. Thus,
  I₁ = (1/2)∫₀^π cos(cosθ)dθ  and  I₂ = (1/2)∫₀^π cos2θ · cos(cosθ)dθ.

Step 5. Using a standard integral representation of Bessel functions

A standard formula (see, e.g., Gradstein–Ryzhik) is that for an even integer n one has
  ∫₀^π cos(nθ) cos(z cosθ)dθ = π (–1)^(n/2) Jₙ(z).
Taking z = 1 we get:
  For n = 0:  ∫₀^π cos(cosθ)dθ = π J₀(1).
  For n = 2:  ∫₀^π cos2θ cos(cosθ)dθ = π (–1)^(1) J₂(1) = –π J₂(1).

Thus,
  I₁ = (π/2) J₀(1),
  I₂ = (1/2)(–π J₂(1)) = – (π/2) J₂(1).

So the overall integral becomes
  I = I₁ + I₂ = (π/2)[J₀(1) – J₂(1)].

Step 6. A numerical approximation

Using standard values for the Bessel functions:
  J₀(1) ≈ 0.7651976866  and  J₂(1) ≈ 0.1149034849,
we have
  J₀(1) – J₂(1) ≈ 0.6502942017.
Thus,
  I ≈ (π/2) × 0.6502942017.
Since π/2 ≈ 1.5707963268, it follows that
  I ≈ 1.5707963268 × 0.6502942017 ≈ 1.0210176120.

Final answer in JSON format:
{"answer": "$(\\frac{\\pi}{2})(J_0(1)-J_2(1))$", "numerical_answer": "1.0210176120"}