Let us compute the integral:
\[
I = \int_0^\pi \cos(x+\cos{x})\,dx
\]

**Step 1: Analytical Calculation**

Let us attempt substitution or symmetry.

Let \( u = \pi - x \Rightarrow du = -dx \).

When \( x = 0 \), \( u = \pi \).  
When \( x = \pi \), \( u = 0 \).

Thus,
\[
I = \int_{x=0}^{x=\pi} \cos(x+\cos x) dx = \int_{u=\pi}^{u=0} \cos((\pi-u)+\cos(\pi-u)) (-du)
\]
which reverses the endpoints:
\[
= \int_{u=0}^{u=\pi} \cos((\pi-u)+\cos(\pi-u)) du
\]
Next,
\[
\cos(\pi-u) = -\cos u
\]
So:
\[
(\pi-u) + \cos(\pi-u) = \pi-u - \cos u
\]

Thus,
\[
I = \int_{0}^{\pi} \cos(\pi - u - \cos u) du
\]
Recall that \(\cos(\pi - \theta) = -\cos \theta\), so
\[
I = \int_0^\pi -\cos(u+\cos u) du = -I
\]
So,
\[
I = -I \implies I = 0
\]

**Step 2: All steps are shown above.**

**Step 3: Numerical Approximation**

So the numerical result is 0.

**Step 4: JSON formatted answer**

```json
{"answer": "0", "numerical_answer": "0.0000000000"}
```