Let us compute 
\[
I = \int_{0}^{2} x \arctan\left(\sqrt{x(2-x)}\right) dx
\]

**Step 1: Substitution**

Let’s use the substitution \( x = 2 \sin^2 \theta \), for \( \theta \in [0, \pi/2] \):

- When \( x = 0 \), \( \theta = 0 \)
- When \( x = 2 \), \( \sin^2\theta = 1 \implies \theta = \frac{\pi}{2} \)
- \( dx = 4 \sin\theta \cos\theta d\theta = 2 \sin 2\theta d\theta \)

Compute the inside of the arctan:
\[
x(2-x) = 2\sin^2\theta (2 - 2\sin^2\theta) = 4\sin^2\theta \cos^2\theta = \sin^2 2\theta
\]
\[
\sqrt{x(2-x)} = |\sin 2\theta|
\]
On \( [0, \pi/2] \), \( \sin 2\theta \ge 0 \), so \( \sqrt{x(2-x)} = \sin 2\theta \) directly.

So \( x = 2\sin^2\theta \), \( dx = 2\sin 2\theta d\theta \)

Plug in:

\[
I = \int_0^{\pi/2} [2\sin^2\theta]\, \arctan(\sin 2\theta)\, [2\sin 2\theta d\theta]
= 4 \int_0^{\pi/2} \sin^2\theta \sin 2\theta \arctan(\sin 2\theta) d\theta
\]

Recall \( \sin^2\theta \sin 2\theta = 2 \sin^3\theta \cos\theta \):

\[
I = 8 \int_{0}^{\pi/2} \sin^3\theta \cos\theta\, \arctan(\sin 2\theta)\, d\theta
\]

**Step 2: Substitute \( u = \sin 2\theta \) (optional check)**

Let’s try to write the integral in terms of \( t = \sin 2\theta \), but \(\sin^3\theta\) and \(\cos\theta\) do not transform conveniently. Instead, we try integration by parts.

Let:
\[
u = \arctan(\sin 2\theta), \quad dv = \sin^3\theta \cos\theta d\theta
\]
Then
\[
du = \frac{2\cos 2\theta}{1+\sin^2 2\theta} d\theta
\]
\[
v = \int \sin^3\theta \cos\theta d\theta
\]

Let’s compute \( \int \sin^3\theta \cos\theta d\theta \):

Let \( w = \sin\theta \), \( dw = \cos\theta d\theta \), so

\[
\int \sin^3\theta \cos\theta d\theta = \int w^3 dw = \frac{w^4}{4} = \frac{\sin^4\theta}{4}
\]

Therefore,
\[
I = 8 \left[ \frac{\sin^4\theta}{4}\arctan(\sin 2\theta) \Bigg|_0^{\pi/2}
- \int_0^{\pi/2} \frac{\sin^4\theta}{4} \cdot \frac{2\cos 2\theta}{1 + \sin^2 2\theta} d\theta \right]
\]

\[
= 2 \left[ \sin^4\theta\, \arctan(\sin 2\theta) \Big|_0^{\pi/2}
- 2 \int_0^{\pi/2} \frac{\sin^4\theta\, \cos 2\theta}{1 + \sin^2 2\theta} d\theta \right]
\]

Now, evaluate the boundary term:

- At \( \theta = 0, \sin\theta = 0 \implies 0 \)
- At \( \theta = \pi/2, \sin\theta = 1 \), \( \sin 2\theta = 0 \), so \( \arctan(0) = 0 \), so boundary term is zero.

Therefore,

\[
I = -4 \int_0^{\pi/2} \frac{\sin^4\theta\, \cos 2\theta}{1 + \sin^2 2\theta} d\theta
\]

**Now, \(\sin^4\theta\) and \(\cos 2\theta\)**

Let us write \( \sin^4\theta \) in terms of multiple angles:

\[
\sin^4\theta = \left(\sin^2\theta\right)^2 = \left(\frac{1 - \cos 2\theta}{2}\right)^2
= \frac{1}{4}(1 - 2\cos 2\theta + \cos^2 2\theta)
\]

\( \cos^2 2\theta = \frac{1+\cos 4\theta}{2} \)

So,

\[
\sin^4\theta = \frac{1}{4} \left(1 - 2\cos 2\theta + \frac{1 + \cos 4\theta}{2}\right)
= \frac{1}{4} \left(\frac{3}{2} - 2\cos 2\theta + \frac{1}{2} \cos 4\theta\right)
\]

But let's use \( \sin^4\theta = \frac{3}{8} - \frac{1}{2} \cos 2\theta + \frac{1}{8} \cos 4\theta \):

\[
\sin^4\theta = \frac{3}{8} - \frac{1}{2} \cos 2\theta + \frac{1}{8} \cos 4\theta
\]

Now,

\[
I = -4 \int_0^{\pi/2} \frac{ 
\left( \frac{3}{8} - \frac{1}{2} \cos 2\theta + \frac{1}{8} \cos 4\theta \right) 
\cos 2\theta 
}{1 + \sin^2 2\theta} d\theta
\]
\[
= -4 \left[ \frac{3}{8} \int_0^{\pi/2} \frac{ \cos 2\theta }{1 + \sin^2 2\theta} d\theta
- \frac{1}{2} \int_0^{\pi/2} \frac{ \cos^2 2\theta }{1 + \sin^2 2\theta} d\theta
+ \frac{1}{8} \int_0^{\pi/2} \frac{ \cos 2\theta \cos 4\theta }{1 + \sin^2 2\theta} d\theta
\right]
\]

Let us call these \( I_1, I_2, I_3 \):

\[
I = -4 \left( \frac{3}{8} I_1 - \frac{1}{2} I_2 + \frac{1}{8} I_3 \right )
\]

where

\[
I_1 = \int_0^{\pi/2} \frac{ \cos 2\theta }{1 + \sin^2 2\theta} d\theta
\qquad
I_2 = \int_0^{\pi/2} \frac{ \cos^2 2\theta }{1 + \sin^2 2\theta} d\theta
\qquad
I_3 = \int_0^{\pi/2} \frac{ \cos 2\theta \cos 4\theta }{1 + \sin^2 2\theta} d\theta
\]

Let’s compute these one by one.

---

# Computation of \(I_1\):

Let \( u = 2\theta \), \( du = 2 d\theta \), as \( \theta \) goes from 0 to \( \pi/2 \), \( u \) goes from 0 to \( \pi \):

\[
I_1 = \int_0^{\pi/2} \frac{ \cos 2\theta }{1 + \sin^2 2\theta} d\theta
= \frac{1}{2} \int_0^{\pi} \frac{ \cos u }{1 + \sin^2 u } du 
\]

Note that \( f(u) = \cos u/(1 + \sin^2 u) \) is an odd function about \( u = \pi/2 \), due to \( \cos(\pi - x) = -\cos x \) and \( \sin^2 (\pi - x) = \sin^2 x \). Therefore, over \( [0, \pi] \), integrating this function yields 0.

So,

\[
I_1 = 0
\]

---

# Computation of \(I_2\):

\[
I_2 = \int_0^{\pi/2} \frac{ \cos^2 2\theta }{1 + \sin^2 2\theta} d\theta
\]
Let \( \cos^2 2\theta = 1 - \sin^2 2\theta \):

\[
I_2 = \int_0^{\pi/2} \frac{ 1 - \sin^2 2\theta }{ 1 + \sin^2 2\theta } d\theta
= \int_0^{\pi/2} \left( \frac{1 + \sin^2 2\theta - 2\sin^2 2\theta }{ 1 + \sin^2 2\theta } \right) d\theta
= \int_0^{\pi/2} \left( 1 - \frac{2\sin^2 2\theta }{1 + \sin^2 2\theta} \right) d\theta
\]

Therefore,
\[
I_2 = \int_0^{\pi/2} d\theta - 2\int_0^{\pi/2} \frac{\sin^2 2\theta}{1 + \sin^2 2\theta} d\theta
\]
\[
= \frac{\pi}{2} - 2 J
\]
where \( J = \int_0^{\pi/2} \frac{\sin^2 2\theta}{1 + \sin^2 2\theta} d\theta \).

Let’s compute \( J \):

But
\[
\frac{\sin^2 2\theta}{1 + \sin^2 2\theta} = 1 - \frac{1}{1 + \sin^2 2\theta}
\]
So
\[
J = \int_0^{\pi/2} \left( 1 - \frac{1}{1 + \sin^2 2\theta} \right) d\theta
= \frac{\pi}{2} - K
\]
where \( K = \int_0^{\pi/2} \frac{ d\theta }{1 + \sin^2 2\theta} \)

Therefore,
\[
I_2 = \frac{\pi}{2} - 2J = \frac{\pi}{2} - 2\left( \frac{\pi}{2} - K \right ) = -\frac{\pi}{2} + 2K
\]

---

# Computation of \(I_3\):

\[
I_3 = \int_0^{\pi/2} \frac{ \cos 2\theta \cos 4\theta}{1 + \sin^2 2\theta} d\theta
\]
\[
\cos 2\theta \cos 4\theta = \frac{ \cos(2\theta + 4\theta) + \cos(2\theta - 4\theta) }{2 } = \frac{ \cos 6\theta + \cos(-2\theta) }{2 } = \frac{ \cos 6\theta + \cos 2\theta }{2 }
\]

So,

\[
I_3 = \frac{1}{2} \int_0^{\pi/2} \frac{ \cos 6\theta + \cos 2\theta }{ 1 + \sin^2 2\theta } d\theta \\
= \frac{1}{2} \int_0^{\pi/2} \frac{ \cos 6\theta }{1 + \sin^2 2\theta} d\theta + \frac{1}{2} \int_0^{\pi/2} \frac{ \cos 2\theta }{1 + \sin^2 2\theta } d\theta
\]

The last term is just \(I_1 = 0\).

Let us denote
\[
I_3 = \frac{1}{2} \int_0^{\pi/2} \frac{ \cos 6\theta }{1 + \sin^2 2\theta} d\theta
\]
But \( \int_0^{\pi/2} \frac{ \cos 6\theta }{1 + \sin^2 2\theta } d\theta = 0 \) by a symmetric argument: \(\cos 6\theta\) averages to zero times an even function.

Let us check this:

Let \( \sin^2 2(\frac{\pi}{2}-\theta) = \sin^2(\pi - 2\theta) = \sin^2 2\theta \), and \( \cos 6(\frac{\pi}{2}-\theta) = \cos (3\pi - 6\theta) = -\cos 6\theta \). Therefore the integral is antisymmetric about \( \theta = \pi/4 \):

\[
\int_0^{\pi/2} \frac{ \cos 6\theta }{1 + \sin^2 2\theta } d\theta = 0
\]

Therefore, \( I_3 = 0 \).

---

# Gathering everything:

Thus:

\[
I = -4\left[\frac{3}{8}\cdot 0 - \frac{1}{2}\left(-\frac{\pi}{2} + 2K\right) + \frac{1}{8}\cdot 0\right ]
= -4 \left[ \frac{\pi}{4} - K \right ]
= -\pi + 4K
\]
with
\[
K = \int_0^{\pi/2} \frac{ d\theta }{1 + \sin^2 2\theta }
\]

---

# Step 3: Express in terms of standard integrals

Let’s try to simplify \( K \). Let’s use \( \sin^2 2\theta = \frac{1 - \cos 4\theta}{2} \):

\[
K = \int_0^{\pi/2} \frac{ d\theta }{ 1 + \frac{1 - \cos 4\theta}{2} }
= \int_0^{\pi/2} \frac{d\theta}{ \frac{3}{2} - \frac{1}{2} \cos 4\theta }
= 2 \int_0^{\pi/2} \frac{d\theta}{ 3 - \cos 4\theta }
\]

Let’s make substitution \( \phi = 4\theta \), \( \theta = 0 \to \phi = 0 \), \( \theta = \pi/2 \to \phi = 2\pi \), \( d\theta = d\phi/4 \):

\[
K = 2 \int_0^{\pi/2} \frac{d\theta}{3 - \cos 4\theta }
= 2 \int_0^{2\pi} \frac{d\phi}{4[3 - \cos\phi]}
= \frac{1}{2} \int_0^{2\pi} \frac{ d\phi }{3 - \cos\phi }
\]

So,

\[
K = \frac{1}{2} \int_0^{2\pi} \frac{ d\phi }{3 - \cos\phi }
\]

---

Now, the standard integral:

\[
\int_0^{2\pi} \frac{d\phi}{a - b\cos\phi} = \frac{2\pi}{\sqrt{a^2 - b^2}}
\]
valid when \( |b| < |a| \).

For our case, \( a = 3, b = 1 \):

\[
\int_0^{2\pi} \frac{d\phi}{3 - \cos\phi} = \frac{2\pi}{\sqrt{9 - 1}} = \frac{2\pi}{\sqrt{8}} = \frac{2\pi}{2\sqrt{2}} = \frac{\pi}{\sqrt{2}}
\]

So

\[
K = \frac{1}{2} \cdot \frac{\pi}{\sqrt{2}} = \frac{\pi}{2\sqrt{2}}
\]

---

# Final exact answer

Recall:
\[
I = -\pi + 4K = -\pi + 4 \cdot \frac{\pi}{2\sqrt{2}} = -\pi + \frac{2\pi}{\sqrt{2}} = -\pi + \sqrt{2}\pi = (\sqrt{2}-1)\pi
\]

---

# Step 4: Numerical Approximation

\[
I = (\sqrt{2}-1)\pi \approx (1.4142135623730951 - 1) \cdot 3.1415926535897932 \approx 0.4142135623730951 \times 3.1415926535897932 \approx 1.3012902840
\]

---

# Final Output (JSON format)

```json
{"answer": "(\\sqrt{2}-1)\\pi", "numerical_answer": "1.3012902840"}
```