To solve the definite integral \(\int\limits_{0}^{\infty}\frac{x^{3}}{e^x-1}\left[8\cosh\left(0.5x\right)-\cosh\left(0.25x\right)\right]dx\), we will follow the steps outlined.

### Step 1: Simplify the integrand

First, let's rewrite the integrand using the definition of the hyperbolic cosine function \(\cosh(y) = \frac{e^y + e^{-y}}{2}\):

\[
8\cosh(0.5x) - \cosh(0.25x) = 8 \cdot \frac{e^{0.5x} + e^{-0.5x}}{2} - \frac{e^{0.25x} + e^{-0.25x}}{2}
\]

Simplify the expression:

\[
8\cosh(0.5x) - \cosh(0.25x) = 4(e^{0.5x} + e^{-0.5x}) - \frac{1}{2}(e^{0.25x} + e^{-0.25x})
\]

### Step 2: Split the integral

Now, split the integral into two parts:

\[
\int\limits_{0}^{\infty}\frac{x^{3}}{e^x-1} \left[4(e^{0.5x} + e^{-0.5x}) - \frac{1}{2}(e^{0.25x} + e^{-0.25x})\right] dx
\]

This can be written as:

\[
4 \int\limits_{0}^{\infty}\frac{x^{3} e^{0.5x}}{e^x-1} dx + 4 \int\limits_{0}^{\infty}\frac{x^{3} e^{-0.5x}}{e^x-1} dx - \frac{1}{2} \int\limits_{0}^{\infty}\frac{x^{3} e^{0.25x}}{e^x-1} dx - \frac{1}{2} \int\limits_{0}^{\infty}\frac{x^{3} e^{-0.25x}}{e^x-1} dx
\]

### Step 3: Use known integral results

We use the known result for integrals of the form \(\int\limits_{0}^{\infty} \frac{x^{n} e^{-ax}}{e^x - 1} dx\):

\[
\int\limits_{0}^{\infty} \frac{x^{n} e^{-ax}}{e^x - 1} dx = \Gamma(n+1) \zeta(n+1) \left(1 - \frac{1}{2^{n+1}}\right)
\]

For \(n = 3\):

\[
\int\limits_{0}^{\infty} \frac{x^{3} e^{-ax}}{e^x - 1} dx = 6 \zeta(4) \left(1 - \frac{1}{2^{4}}\right) = 6 \zeta(4) \left(1 - \frac{1}{16}\right) = 6 \zeta(4) \cdot \frac{15}{16}
\]

Since \(\zeta(4) = \frac{\pi^4}{90}\):

\[
\int\limits_{0}^{\infty} \frac{x^{3} e^{-ax}}{e^x - 1} dx = 6 \cdot \frac{\pi^4}{90} \cdot \frac{15}{16} = \frac{6 \cdot 15 \cdot \pi^4}{90 \cdot 16} = \frac{90 \pi^4}{1440} = \frac{\pi^4}{16}
\]

### Step 4: Apply the result to each term

For \(a = 0.5\):

\[
4 \int\limits_{0}^{\infty}\frac{x^{3} e^{-0.5x}}{e^x-1} dx = 4 \cdot \frac{\pi^4}{16} = \frac{\pi^4}{4}
\]

For \(a = -0.5\):

\[
4 \int\limits_{0}^{\infty}\frac{x^{3} e^{0.5x}}{e^x-1} dx = 4 \cdot \frac{\pi^4}{16} = \frac{\pi^4}{4}
\]

For \(a = 0.25\):

\[
-\frac{1}{2} \int\limits_{0}^{\infty}\frac{x^{3} e^{-0.25x}}{e^x-1} dx = -\frac{1}{2} \cdot \frac{\pi^4}{16} = -\frac{\pi^4}{32}
\]

For \(a = -0.25\):

\[
-\frac{1}{2} \int\limits_{0}^{\infty}\frac{x^{3} e^{0.25x}}{e^x-1} dx = -\frac{1}{2} \cdot \frac{\pi^4}{16} = -\frac{\pi^4}{32}
\]

### Step 5: Combine the results

Combine all the terms:

\[
\frac{\pi^4}{4} + \frac{\pi^4}{4} - \frac{\pi^4}{32} - \frac{\pi^4}{32} = \frac{\pi^4}{2} - \frac{\pi^4}{16} = \frac{8\pi^4}{16} - \frac{\pi^4}{16} = \frac{7\pi^4}{16}
\]

### Step 6: Numerical approximation

The numerical approximation of \(\frac{7\pi^4}{16}\) is:

\[
\frac{7 \cdot (3.141592653589793)^4}{16} \approx 164.49340668
\]

### Final Answer

\[
\boxed{
\begin{aligned}
\text{"answer": "}\frac{7\pi^4}{16}\text{"}, \\
\text{"numerical_answer": "164.49340668"}
\end{aligned}
}
\]