We start with the integral

  I = ∫₀∞ [tanh(x) / exp(x)] dx = ∫₀∞ tanh(x) e^(–x) dx.

Step 1. Write tanh(x) in an equivalent form:
  tanh(x) = 1 – [2 / (exp(2x) + 1)].

Thus the integrand becomes:
  tanh(x) e^(–x) = e^(–x) – [2 e^(–x) / (exp(2x) + 1)].

Then the integral splits into two parts:
  I = ∫₀∞ e^(–x) dx – 2 ∫₀∞ [e^(–x) / (exp(2x) + 1)] dx.

Step 2. Evaluate the first integral:
  ∫₀∞ e^(–x) dx = [–e^(–x)]₀∞ = (0 – (–1)) = 1.

Step 3. Rewrite and evaluate the second integral:
Let
  I₂ = ∫₀∞ [e^(–x) / (exp(2x) + 1)] dx.
Write the denominator as exp(2x)+1 = 1+exp(2x) so that:
  1/(exp(2x)+1) = e^(–2x) / (1+e^(–2x)).
Now use the series expansion for 1/(1+e^(–2x)):
  1/(1+e^(–2x)) = Σₙ₌₀∞ [ (–1)ⁿ e^(–2nx) ]   (for |e^(–2x)| < 1, which is valid for x > 0).

Thus,
  I₂ = ∫₀∞ e^(–x) ⋅ e^(–2x) Σₙ₌₀∞ (–1)ⁿ e^(–2nx) dx
    = Σₙ₌₀∞ (–1)ⁿ ∫₀∞ e^(–(2n+3)x) dx.
Each integral is:
  ∫₀∞ e^(–(2n+3)x) dx = 1/(2n+3).

So we have:
  I₂ = Σₙ₌₀∞ (–1)ⁿ/(2n+3).

Step 4. Express the series in closed form:
Express the term 1/(2n+3) as an integral using the formula
  1/(2n+3) = ∫₀¹ t^(2n+2) dt.
Then,
  I₂ = Σₙ₌₀∞ (–1)ⁿ ∫₀¹ t^(2n+2) dt = ∫₀¹ t² Σₙ₌₀∞ (–1)ⁿ t^(2n) dt.
Recognize the inner sum as a geometric series:
  Σₙ₌₀∞ (–1)ⁿ t^(2n) = 1/(1+t²)  (for |t|<1, and the integration is over [0,1] so it is valid).

Thus,
  I₂ = ∫₀¹ [t²/(1+t²)] dt.
Simplify the integrand by writing:
  t²/(1+t²) = 1 – [1/(1+t²)].
Now integrate term‐by‐term:
  ∫₀¹ 1 dt = 1  and  ∫₀¹ 1/(1+t²) dt = arctan(t)|₀¹ = π/4.
Thus,
  I₂ = 1 – (π/4).

Step 5. Combine the results:
Recall that
  I = 1 – 2 I₂ = 1 – 2[1 – (π/4)] = 1 – 2 + (π/2) = (π/2) – 1.

Step 6. Numerical approximation:
Substitute π ≈ 3.141592653589793, then
  (π/2) – 1 ≈ (1.5707963267948966 – 1) = 0.5707963267948966.
Rounded to 10 decimal places, this is 0.5707963268.

Final Answer in JSON format:
{"answer": "\\frac{\\pi}{2} - 1", "numerical_answer": "0.5707963268"}