We wish to evaluate

  I = ∫₀² x^(–1/2) (2–x)^(–1/2) cosh(√(x(2–x))) dx.

Step 1. Change of Variables

A good substitution is
  x = 1 – cosθ.
When x = 0, we have 0 = 1 – cosθ so cosθ = 1 and thus θ = 0.
When x = 2, 2 = 1 – cosθ so cosθ = –1 and hence θ = π.

Differentiate:
  dx = sinθ dθ.

Also, notice that
  2–x = 2 – (1 – cosθ) = 1 + cosθ.
and
  √(x(2–x)) = √((1–cosθ)(1+cosθ)) = √(1–cos²θ) = sinθ   (since 0 ≤ θ ≤ π so sinθ ≥ 0).

Now, the factors in the integrand become
  x^(–1/2)(2–x)^(–1/2) = 1/√(x(2–x)) = 1/sinθ.
Thus, dx/(√(x(2–x))) = (sinθ dθ)/(sinθ) = dθ.
Also, cosh(√(x(2–x))) becomes cosh(sinθ).

Thus the integral transforms into
  I = ∫₀^π cosh(sinθ) dθ.

Step 2. Expressing the Integral in a Closed Form

Now we have
  I = ∫₀^π cosh(sinθ)dθ.
A powerful way to attack this is to use a Fourier expansion. Notice that
  cosh(sinθ) = cos(i sinθ)   (since cosh(t) = cos(it)).
A standard expansion (the Jacobi–Anger expansion) for the cosine of a sine is
  cos(z sinθ) = J₀(z) + 2∑ₘ₌₁∞ J₂ₘ(z) cos(2mθ),
where Jₙ(z) is the Bessel function of order n.

Setting z = i we get
  cosh(sinθ) = cos(i sinθ) = J₀(i) + 2∑ₘ₌₁∞ J₂ₘ(i) cos(2mθ).
There is a standard relation:
  Jₙ(i) = iⁿ Iₙ(1),
so in particular,
  J₀(i) = I₀(1)   and  J₂ₘ(i) = i^(2m) I₂ₘ(1) = I₂ₘ(1).
Thus,
  cosh(sinθ) = I₀(1) + 2∑ₘ₌₁∞ I₂ₘ(1) cos(2mθ).

Integrate from 0 to π:
  I = ∫₀^π cosh(sinθ)dθ = I₀(1)∫₀^π dθ + 2∑ₘ₌₁∞ I₂ₘ(1) ∫₀^π cos(2mθ)dθ.
But for m ≥ 1, ∫₀^π cos(2mθ)dθ = 0. Hence only the m = 0 term survives and we get
  I = π I₀(1).

Step 3. Numerical Approximation

The modified Bessel function I₀(1) is known to be approximately
  I₀(1) ≈ 1.2660658777520082.
Thus,
  I ≈ π × 1.2660658777520082 ≈ 3.9762698690
(to 10 decimal places).

Step 4. Final Answer in JSON Format

{"answer": "$\\pi I_0(1)$", "numerical_answer": "3.9762698690"}