To compute the definite integral \(\int_0^\infty \frac{1}{e^x + 1} \, dx\), we can proceed with the following steps:

### Step 1: Substitution
Let \( u = e^x \). Then, \( du = e^x dx \) or \( dx = \frac{du}{u} \). When \( x = 0 \), \( u = 1 \), and as \( x \to \infty \), \( u \to \infty \). The integral becomes:

\[
\int_0^\infty \frac{1}{e^x + 1} \, dx = \int_1^\infty \frac{1}{u + 1} \cdot \frac{du}{u}
\]

### Step 2: Partial Fractions
We can rewrite the integrand using partial fractions:

\[
\frac{1}{u(u + 1)} = \frac{1}{u} - \frac{1}{u + 1}
\]

Thus, the integral becomes:

\[
\int_1^\infty \left( \frac{1}{u} - \frac{1}{u + 1} \right) du
\]

### Step 3: Integrate
Now, integrate term by term:

\[
\int_1^\infty \frac{1}{u} \, du - \int_1^\infty \frac{1}{u + 1} \, du
\]

The first integral is:

\[
\int_1^\infty \frac{1}{u} \, du = \ln u \Big|_1^\infty = \lim_{u \to \infty} \ln u - \ln 1 = \infty - 0 = \infty
\]

However, this suggests that the integral diverges, which contradicts our expectation. Let's re-examine the substitution step.

### Correct Approach: Alternative Substitution
Instead, let’s use the substitution \( v = e^x + 1 \). Then, \( dv = e^x dx = (v - 1) dx \), so \( dx = \frac{dv}{v - 1} \). The limits change as follows: when \( x = 0 \), \( v = 2 \), and as \( x \to \infty \), \( v \to \infty \). The integral becomes:

\[
\int_0^\infty \frac{1}{e^x + 1} \, dx = \int_2^\infty \frac{1}{v} \cdot \frac{dv}{v - 1}
\]

This seems more complicated. Let’s try another approach.

### Step 4: Series Expansion
We can express \(\frac{1}{e^x + 1}\) as a series:

\[
\frac{1}{e^x + 1} = \frac{e^{-x}}{1 + e^{-x}} = e^{-x} \sum_{n=0}^\infty (-1)^n e^{-n x} = \sum_{n=0}^\infty (-1)^n e^{-(n + 1)x}
\]

Now, integrate term by term:

\[
\int_0^\infty \sum_{n=0}^\infty (-1)^n e^{-(n + 1)x} \, dx = \sum_{n=0}^\infty (-1)^n \int_0^\infty e^{-(n + 1)x} \, dx
\]

The integral of \( e^{-(n + 1)x} \) is:

\[
\int_0^\infty e^{-(n + 1)x} \, dx = \frac{1}{n + 1}
\]

Thus, the integral becomes:

\[
\sum_{n=0}^\infty \frac{(-1)^n}{n + 1} = \sum_{k=1}^\infty \frac{(-1)^{k - 1}}{k} = \ln 2
\]

This is the alternating harmonic series, which converges to \(\ln 2\).

### Step 5: Numerical Approximation
The numerical value of \(\ln 2\) is approximately:

\[
\ln 2 \approx 0.6931471806
\]

### Final Answer
The exact answer is \(\ln 2\), and its numerical approximation is \(0.6931471806\).

```json
{"answer": "\\ln 2", "numerical_answer": "0.6931471806"}
```