
To solve the definite integral \(\int\limits_0^1 x \mathbf{L}_0(2\sqrt{x}) \mathbf{K}\left(\sqrt{1-x}\right) dx\), we proceed as follows:

### Step 1: Simplify the Laguerre polynomial
The 0th-order Laguerre polynomial \(\mathbf{L}_0(z)\) is identically 1 for all \(z\). Thus, \(\mathbf{L}_0(2\sqrt{x}) = 1\), reducing the integral to:
\[
\int_0^1 x \cdot 1 \cdot \mathbf{K}\left(\sqrt{1-x}\right) dx = \int_0^1 x \mathbf{K}\left(\sqrt{1-x}\right) dx.
\]

### Step 2: Substitution to simplify the integral
Let \(t = \sqrt{1-x}\), so \(t^2 = 1-x\) and \(x = 1-t^2\). Then \(dx = -2t \, dt\). When \(x=0\), \(t=1\); when \(x=1\), \(t=0\). Changing variables, the integral becomes:
\[
\int_{t=1}^0 (1-t^2) \mathbf{K}(t) \cdot (-2t \, dt) = \int_0^1 2t(1-t^2) \mathbf{K}(t) \, dt.
\]

### Step 3: Evaluate the transformed integral
The integral \(\int_0^1 2t(1-t^2) \mathbf{K}(t) \, dt\) can be split into two parts:
\[
2 \int_0^1 t \mathbf{K}(t) \, dt - 2 \int_0^1 t^3 \mathbf{K}(t) \, dt.
\]

### Step 4: Use known results for integrals involving \(\mathbf{K}(t)\)
From standard integral results involving the complete elliptic integral of the first kind \(\mathbf{K}(t)\):
- \(\int_0^1 t \mathbf{K}(t) \, dt = \frac{\pi}{4}\),
- \(\int_0^1 t^3 \mathbf{K}(t) \, dt = \frac{\pi}{16}\).

### Step 5: Combine the results
Substituting these into the expression:
\[
2 \left( \frac{\pi}{4} - \frac{\pi}{16} \right) = 2 \cdot \frac{3\pi}{16} = \frac{3\pi}{8}.
\]

### Numerical Approximation
The numerical value of \(\frac{3\pi}{8}\) is approximately \(1.1780972451\) (rounded to 10 decimal places).

### Final Answer
{"answer": "\\frac{3\\pi}{8}", "numerical_answer": "1.1780972451"}