# Evaluating $\int_0^1\sqrt[3]{x}\left\lfloor\frac1{\sqrt[3]{x}}\right\rfloor\:\mathrm{d}x$

Let's start by making a substitution to simplify this integral.

## Step 1: Substitution
Let $u = x^{1/3}$, then $x = u^3$ and $dx = 3u^2 du$.

When $x = 0$, $u = 0$
When $x = 1$, $u = 1$

The integral becomes:
$$\int_0^1 x^{1/3} \left\lfloor\frac{1}{x^{1/3}}\right\rfloor\:\mathrm{d}x = \int_0^1 u \left\lfloor\frac{1}{u}\right\rfloor \cdot 3u^2 \:\mathrm{d}u = 3 \int_0^1 u^3 \left\lfloor\frac{1}{u}\right\rfloor \:\mathrm{d}u$$

## Step 2: Analyze the floor function
For $0 < u \leq 1$, we need to determine $\left\lfloor\frac{1}{u}\right\rfloor$.

The function $\frac{1}{u}$ takes the following values:
- For $\frac{1}{2} < u \leq 1$, we have $1 \leq \frac{1}{u} < 2$, so $\left\lfloor\frac{1}{u}\right\rfloor = 1$
- For $\frac{1}{3} < u \leq \frac{1}{2}$, we have $2 \leq \frac{1}{u} < 3$, so $\left\lfloor\frac{1}{u}\right\rfloor = 2$
- For $\frac{1}{4} < u \leq \frac{1}{3}$, we have $3 \leq \frac{1}{u} < 4$, so $\left\lfloor\frac{1}{u}\right\rfloor = 3$

And so on. In general, for $\frac{1}{n+1} < u \leq \frac{1}{n}$, we have $\left\lfloor\frac{1}{u}\right\rfloor = n$.

## Step 3: Split the integral
We need to split the integral into parts where $\left\lfloor\frac{1}{u}\right\rfloor$ has a constant value:

$$3 \int_0^1 u^3 \left\lfloor\frac{1}{u}\right\rfloor \:\mathrm{d}u = 3 \sum_{n=1}^{\infty} n \int_{\frac{1}{n+1}}^{\frac{1}{n}} u^3 \:\mathrm{d}u$$

## Step 4: Evaluate each part
For each segment, we evaluate:

$$\int_{\frac{1}{n+1}}^{\frac{1}{n}} u^3 \:\mathrm{d}u = \left. \frac{u^4}{4} \right|_{\frac{1}{n+1}}^{\frac{1}{n}} = \frac{1}{4} \left[ \frac{1}{n^4} - \frac{1}{(n+1)^4} \right]$$

## Step 5: Compute the sum
Our integral becomes:

$$3 \sum_{n=1}^{\infty} n \cdot \frac{1}{4} \left[ \frac{1}{n^4} - \frac{1}{(n+1)^4} \right] = \frac{3}{4} \sum_{n=1}^{\infty} \left[ \frac{n}{n^4} - \frac{n}{(n+1)^4} \right]$$

$$= \frac{3}{4} \sum_{n=1}^{\infty} \left[ \frac{1}{n^3} - \frac{n}{(n+1)^4} \right]$$

## Step 6: Simplify and calculate
Let's work with the second term in the sum:

$$\frac{n}{(n+1)^4} = \frac{n+1-1}{(n+1)^4} = \frac{n+1}{(n+1)^4} - \frac{1}{(n+1)^4} = \frac{1}{(n+1)^3} - \frac{1}{(n+1)^4}$$

So our sum becomes:

$$\frac{3}{4} \sum_{n=1}^{\infty} \left[ \frac{1}{n^3} - \frac{1}{(n+1)^3} + \frac{1}{(n+1)^4} \right]$$

The sum of $\frac{1}{n^3} - \frac{1}{(n+1)^3}$ is a telescoping series. When we add all terms, only $\frac{1}{1^3} = 1$ remains.

Our integral equals:
$$\frac{3}{4} \left[ 1 + \sum_{n=1}^{\infty} \frac{1}{(n+1)^4} \right] = \frac{3}{4} \left[ 1 + \sum_{k=2}^{\infty} \frac{1}{k^4} \right]$$

$$= \frac{3}{4} \left[ 1 + \left(\sum_{k=1}^{\infty} \frac{1}{k^4} - 1\right) \right] = \frac{3}{4} \cdot \sum_{k=1}^{\infty} \frac{1}{k^4}$$

The sum $\sum_{k=1}^{\infty} \frac{1}{k^4} = \zeta(4) = \frac{\pi^4}{90}$

Therefore:
$$\int_0^1\sqrt[3]{x}\left\lfloor\frac1{\sqrt[3]{x}}\right\rfloor\:\mathrm{d}x = \frac{3}{4} \cdot \frac{\pi^4}{90} = \frac{\pi^4}{120}$$

## Numerical approximation
The numerical value of $\frac{\pi^4}{120}$ is approximately 0.8115920547.

{"answer": "\\frac{\\pi^4}{120}", "numerical_answer": "0.8115920547"}