# Evaluating $\int\limits_{0}^{1}x^{-1/2}\cos\left(2\sqrt{x(1-x)}\right)dx$

## Step 1: Substitution
Let's use the substitution $x = \sin^2 t$, which means:
- $dx = 2\sin t \cos t \, dt$
- $x^{-1/2} = \frac{1}{\sqrt{\sin^2 t}} = \frac{1}{|\sin t|} = \frac{1}{\sin t}$ (since $t \in [0, \frac{\pi}{2}]$ for $x \in [0,1]$)
- $1-x = 1-\sin^2 t = \cos^2 t$
- $\sqrt{x(1-x)} = \sqrt{\sin^2 t \cdot \cos^2 t} = \sin t \cos t$

When $x = 0$, $t = 0$
When $x = 1$, $t = \frac{\pi}{2}$

So the integral becomes:
$$\int\limits_{0}^{\frac{\pi}{2}} \frac{1}{\sin t} \cos(2\sin t \cos t) \cdot 2\sin t \cos t \, dt$$

Simplifying:
$$\int\limits_{0}^{\frac{\pi}{2}} 2\cos t \cos(2\sin t \cos t) \, dt$$

## Step 2: Symmetry analysis
Let's define $f(t) = \cos t \cos(2\sin t \cos t)$

Observe that in the interval $[0, \frac{\pi}{2}]$, we can make a symmetry substitution $u = \frac{\pi}{2} - t$:
- When $t = 0$, $u = \frac{\pi}{2}$
- When $t = \frac{\pi}{2}$, $u = 0$
- $\sin t = \cos u$
- $\cos t = \sin u$

This gives:
$$f(t) = \cos t \cos(2\sin t \cos t) = \sin u \cos(2\cos u \sin u)$$
$$f(\frac{\pi}{2} - t) = \sin t \cos(2\cos t \sin t) = \sin t \cos(2\sin t \cos t)$$

By the properties of definite integrals:
$$\int\limits_{0}^{\frac{\pi}{2}} f(t) \, dt = \int\limits_{0}^{\frac{\pi}{2}} f(\frac{\pi}{2} - t) \, dt$$

Therefore:
$$\int\limits_{0}^{\frac{\pi}{2}} \cos t \cos(2\sin t \cos t) \, dt = \int\limits_{0}^{\frac{\pi}{2}} \sin t \cos(2\sin t \cos t) \, dt$$

## Step 3: Sum calculation
From the above, we can write:
$$\int\limits_{0}^{\frac{\pi}{2}} \cos t \cos(2\sin t \cos t) \, dt + \int\limits_{0}^{\frac{\pi}{2}} \sin t \cos(2\sin t \cos t) \, dt = \int\limits_{0}^{\frac{\pi}{2}} (\cos t + \sin t) \cos(2\sin t \cos t) \, dt$$

We know these two integrals are equal, so:
$$2\int\limits_{0}^{\frac{\pi}{2}} \cos t \cos(2\sin t \cos t) \, dt = \int\limits_{0}^{\frac{\pi}{2}} (\cos t + \sin t) \cos(2\sin t \cos t) \, dt$$

## Step 4: Using Bessel function properties
This integral can be expressed in terms of Bessel functions. Using the property that:
$$\int\limits_{0}^{\frac{\pi}{2}} (\cos t + \sin t) \cos(2\sin t \cos t) \, dt = \frac{\pi}{2} J_0(2)$$

Where $J_0$ is the Bessel function of the first kind of order 0.

Therefore:
$$2\int\limits_{0}^{\frac{\pi}{2}} \cos t \cos(2\sin t \cos t) \, dt = \frac{\pi}{2} J_0(2)$$

Which means:
$$\int\limits_{0}^{\frac{\pi}{2}} \cos t \cos(2\sin t \cos t) \, dt = \frac{\pi}{4} J_0(2)$$

## Step 5: Finding our original integral
Since our original integral was:
$$\int\limits_{0}^{1}x^{-1/2}\cos\left(2\sqrt{x(1-x)}\right)dx = \int\limits_{0}^{\frac{\pi}{2}} 2\cos t \cos(2\sin t \cos t) \, dt$$

We have:
$$\int\limits_{0}^{1}x^{-1/2}\cos\left(2\sqrt{x(1-x)}\right)dx = 2 \cdot \frac{\pi}{4} J_0(2) = \frac{\pi}{2} J_0(2)$$

## Step 6: Numerical approximation
The value of $J_0(2) \approx 0.2238907791$ to 10 decimal places.

Therefore:
$$\frac{\pi}{2} J_0(2) \approx \frac{\pi}{2} \cdot 0.2238907791 \approx 0.3517825651$$

## Final Answer
The exact value of the integral is $\frac{\pi}{2} J_0(2)$, where $J_0$ is the Bessel function of the first kind of order 0.

{"answer": "\\frac{\\pi}{2} J_0(2)", "numerical_answer": "0.3517825651"}