We will show that the integral

  I = ∫₀² x^(–1/2) I₀( x(2–x)^(1/4) ) dx

(with I₀ denoting the modified Bessel function of order 0 and where the fourth root applies to x(2–x)) can be written in closed‐form. (For clarity we write

  I = ∫₀² x^(–1/2) I₀( [x(2–x)]^(1/4) ) dx.)

Step 1. (A Change of Variable)

A very useful substitution is 
  x = 2 sin²θ, with θ ∈ [0, π/2].
Then one computes:
  dx = 4 sinθ cosθ dθ,
  x^(–1/2) = (2 sin²θ)^(–1/2) = 1/(√2 sinθ),
and also
  2 – x = 2 – 2 sin²θ = 2 cos²θ.
Thus
  x(2–x) = 2 sin²θ · 2 cos²θ = 4 sin²θ cos²θ.
Taking the fourth root gives
  [x(2–x)]^(1/4) = (4 sin²θ cos²θ)^(1/4) = (4)^(1/4) (sinθ cosθ)^(1/2)
               = √2 (sinθ cosθ)^(1/2).
Therefore the integrand becomes
  x^(–1/2) I₀([x(2–x)]^(1/4)) dx
   = [1/(√2 sinθ)] · I₀(√2 (sinθ cosθ)^(1/2)) · 4 sinθ cosθ dθ
   = (4 cosθ/√2) I₀(√2 (sinθ cosθ)^(1/2)) dθ
   = 2√2 cosθ I₀(√2 (sinθ cosθ)^(1/2)) dθ.
Thus the transformed integral is
  I = 2√2 ∫₀^(π/2) cosθ I₀(√2 (sinθ cosθ)^(1/2)) dθ.

Step 2. (Rewriting and Series Expansion)

It is not obvious from the integral above that one may “sum it up” immediately. However, one may attack the original I by writing the series expansion for I₀. Recall that

  I₀(z) = Σ (from k=0 to ∞) [ (z/2)^(2k) ]/(k!)².
Thus, with z = [x(2–x)]^(1/4) we get
  I₀([x(2–x)]^(1/4)) = Σₖ₌₀^∞ 1/(k!)² (1/2)^(2k) [x(2–x)]^(k/2).
So
  I = ∫₀² x^(–1/2) Σₖ₌₀^∞ 1/(k!)² (1/2)^(2k) [x(2–x)]^(k/2) dx.
Interchange the sum and the integral (which may be justified under standard convergence theorems):
  I = Σₖ₌₀^∞ 1/(k!)² (1/2)^(2k) ∫₀² x^(k/2 – 1/2) (2–x)^(k/2) dx.
Now make the substitution x = 2u so that dx = 2 du and u runs from 0 to 1. Then
  x^(k/2 – 1/2) = (2u)^(k/2 – 1/2),
  (2–x)^(k/2) = (2(1–u))^(k/2),
and
  ∫₀² x^(k/2 – 1/2) (2–x)^(k/2) dx = 2^( (k/2 – 1/2) + (k/2) + 1 ) ∫₀¹ u^(k/2 – 1/2) (1–u)^(k/2) du.
Notice that the exponent on 2 is
  (k/2 – 1/2) + (k/2) + 1 = k + 1/2.
The remaining u–integral is recognized as a beta–integral:
  B(k/2 + 1/2, k/2 + 1) = Γ(k/2 + 1/2) Γ(k/2 + 1) / Γ(k + 3/2).
Thus we have
  I = Σₖ₌₀^∞ 1/(k!)² (1/2)^(2k) 2^(k+1/2) [Γ(k/2 + 1/2) Γ(k/2 + 1)]/Γ(k + 3/2).
Observe that the factor
  (1/2)^(2k) 2^(k+1/2) = 2^(k+1/2 – 2k) = 2^(1/2 – k).
So
  I = 2^(1/2) Σₖ₌₀^∞ [1/(k!)² 2^(–k) Γ(k/2 + 1/2) Γ(k/2 + 1)]/Γ(k + 3/2).

Step 3. (Using a Gamma–Function Duplication Formula)

A standard relation (see, e.g., formula 5.6.5 in classical references) is
  Γ(z) Γ(z + 1/2) = 2^(1 – 2z) √π Γ(2z).
Take z = (k+1)/2. Then
  Γ((k+1)/2) Γ((k+2)/2) = 2^(1 – (k+1)) √π Γ(k+1)
         = 2^(–k) √π Γ(k+1).
But note that Γ((k+2)/2) = Γ(k/2 + 1), and Γ((k+1)/2) is as it appears. Hence
  Γ(k/2 + 1/2) Γ(k/2 + 1) = 2^(–k) √π · Γ(k+1).
Since Γ(k+1) = k!, we have
  Γ(k/2 + 1/2) Γ(k/2 + 1) = 2^(–k) √π (k!).
Thus the series becomes
  I = 2^(1/2) Σₖ₌₀^∞ [ 1/(k!)² 2^(–k) · 2^(–k) √π (k!) ]/Γ(k+3/2)
    = √{2π} Σₖ₌₀^∞ [1/(k!) 2^(–2k)]/Γ(k+3/2).

But now notice that the confluent hypergeometric limit function {}₀F₁ is defined by
  {}₀F₁(; ν; z) = Σₖ₌₀^∞ zᵏ/(k! Γ(k+ν)).
Comparing with our series we see with ν = 3/2 and z = 1/4 that
  Σₖ₌₀^∞ (1/4)ᵏ/(k! Γ(k+3/2)) = {}₀F₁(; 3/2; 1/4).
Thus we may write
  I = √(2π) · {}₀F₁(; 3/2; 1/4).

Step 4. (Expressing {}₀F₁ in Terms of a Bessel Function)

There is a well‐known relation (see, e.g., Watson’s treatise on Bessel functions) that
  {}₀F₁(; ν; z) = Γ(ν) (z)^{(1–ν)/2} I_{ν–1}(2√z)/( (2√z)^{ν–1} ).
For our case we set ν = 3/2 and z = 1/4. (Note that 2√z = 2√(1/4) = 1.) Then
  {}₀F₁(; 3/2; 1/4)
   = Γ(3/2) (1/4)^{(1–3/2)/2} I_{1/2}(1)/(1^{1/2})
   = Γ(3/2) (1/4)^(–1/4) I_{1/2}(1).
Now,
  (1/4)^(–1/4) = 4^(1/4) = 2^(1/2),
  Γ(3/2) = √π/2,
and a standard formula gives
  I_{1/2}(1) = √(2/(π·1)) sinh(1) = √(2/π) sinh(1).
Thus,
  {}₀F₁(; 3/2; 1/4) = (√π/2) · 2^(1/2) · √(2/π) sinh(1)
     = (√π/2) · √(4/π) sinh(1)
     = (√π/2) · (2/√π) sinh(1)
     = sinh(1).
Therefore the original integral becomes
  I = √(2π) · sinh(1).

Step 5. (Numerical Evaluation)

We now evaluate the numerical value. We have:
  √(2π) = √(6.283185307179586…) ≈ 2.5066282746,
and
  sinh(1) = (e¹ – e^(–1))/2 ≈ (2.7182818285 – 0.3678794412)/2 ≈ 1.1752011936.
Thus,
  I ≈ 2.5066282746 × 1.1752011936 ≈ 2.9460496109.

Final Answer in JSON Format:
{"answer": "\\sqrt{2\\pi}\\sinh(1)", "numerical_answer": "2.9460496109"}