We wish to evaluate

  I = ∫₋₄⁴ e^(|x|){x} dx,

where {x} denotes the fractional part of x (that is, {x} = x − ⎣x⎦).

Because the integrand is defined piecewise on each unit interval (with different expressions for {x} on negative and nonnegative intervals) it is a good idea to split I into two parts:
  I = I₋ + I₊ ,
where
  I₋ = ∫₋₄⁰ e^(|x|){x} dx  and  I₊ = ∫₀⁴ e^(|x|){x} dx.
Notice that for x < 0 we have |x| = –x and for x ≥ 0 we have |x| = x.

Step 1. Compute I₊

For x in [0, 4) the fractional part of x is {x} = x − ⎣x⎦. It is natural to break the interval [0,4] into unit intervals. For n = 0, 1, 2, 3, on the interval x ∈ [n, n+1) we have {x} = x − n. Hence
  I₊ = Σₙ₌₀³ ∫ₙ^(n+1) e^x (x − n) dx.
Make the substitution u = x − n, so that x = u + n and du = dx. When x runs from n to n+1, u runs from 0 to 1. Then
  ∫ₙ^(n+1) e^x (x − n) dx = e^n ∫₀¹ e^u · u du.
We now compute
  I₀ = ∫₀¹ u e^u du.
Integrate by parts:
  Let A = u ⇒ dA = du,
  and dB = e^u du ⇒ B = e^u.
Then,
  I₀ = [u e^u]₀¹ − ∫₀¹ e^u du = [1·e − 0] − (e^u|₀¹) = e − (e − 1) = 1.
Thus, for each interval,
  ∫ₙ^(n+1) e^x (x − n) dx = e^n · 1 = e^n.
So the positive-side contribution is
  I₊ = e⁰ + e¹ + e² + e³ = 1 + e + e² + e³.

Step 2. Compute I₋

For x in [–4, 0) we must be a bit careful with the fractional part. A convenient way is to break the interval [–4, 0) into four unit intervals. For m = 1, 2, 3, 4, consider the interval x ∈ [–m, –m+1). In these intervals the floor is ⎣x⎦ = –m and so
  {x} = x − (–m) = x + m.
Also, since x is negative, |x| = –x. Thus
  I₋ = Σₘ₌₁⁴ ∫₋ₘ^(–m+1) e^(–x) (x + m) dx.
Substitute u = x + m. Then x = u – m and dx = du. When x = –m, u = 0 and when x = –m+1, u = 1. Notice also that
  e^(–x) = e^(–(u – m)) = e^(m – u).
Thus, for each m,
  ∫₋ₘ^(–m+1) e^(–x)(x + m) dx = ∫₀¹ e^(m – u) · u du = e^m ∫₀¹ u e^(–u) du.
Denote
  J₀ = ∫₀¹ u e^(–u) du.
Again we integrate by parts:
  Let C = u ⇒ dC = du,
  and dD = e^(–u) du ⇒ D = –e^(–u).
Thus,
  J₀ = [–u e^(–u)]₀¹ + ∫₀¹ e^(–u) du = (–1·e^(–1) + 0) + (1 – e^(–1)) = 1 − 2e^(–1).
Thus each interval contributes
  e^m (1 − 2/e)     (since e^(–1) = 1/e).
Summing over m = 1, 2, 3, 4 gives
  I₋ = (1 − 2/e) (e + e² + e³ + e⁴).

Step 3. Combine I₊ and I₋

Thus the entire integral is
  I = I₊ + I₋
    = [1 + e + e² + e³] + (1 − 2/e)[e + e² + e³ + e⁴].

Notice that the expression e + e² + e³ + e⁴ appears in I₋; in fact, write:
  (1 − 2/e)(e + e² + e³ + e⁴) = (e + e²+ e³+ e⁴) − (2/e)(e + e²+ e³+ e⁴).
But observe that
  (2/e)(e + e²+ e³+ e⁴) = 2 (1 + e + e²+ e³).
So we have
  I = [1 + e + e² + e³] + (e + e² + e³+ e⁴) − 2(1 + e + e²+ e³)
    = (e + e²+ e³+ e⁴) − (1 + e+ e²+ e³)
    = e⁴ − 1.
Thus, the exact answer is
  I = e⁴ − 1.

Step 4. Numerical Approximation

We use that e⁴ ≈ 54.598150033144236. Thus, numerically,
  I ≈ 54.598150033144236 − 1 = 53.598150033144236.
Rounded to 10 decimal places, this is 53.5981500331.

The final answer in the required JSON format is:
{"answer": "$e^4 - 1$", "numerical_answer": "53.5981500331"}