<think>
Okay, so I need to compute the definite integral from 0 to π of sec(x) times the natural logarithm of (1 + cos(x)/3) dx. Hmm, let's see. First, let me write down the integral properly:

∫₀^π sec(x) ln(1 + (cos x)/3) dx.

Alright, step one is to figure out how to approach this analytically. The integrand is sec(x) multiplied by a logarithm function that includes cos(x). That seems a bit tricky. Let me recall some integration techniques. Maybe substitution? Integration by parts? Or perhaps expanding the logarithm into a series?

Let me think about substitution first. The presence of sec(x) and cos(x) might suggest some trigonometric identity. Remember that sec(x) is 1/cos(x), so maybe that can simplify things. Let's rewrite the integrand:

sec(x) ln(1 + cos(x)/3) = (1/cos(x)) ln(1 + (cos x)/3).

Hmm, so that's [ln(1 + (cos x)/3)] / cos(x). Not sure if that helps yet. Maybe integration by parts? Let's consider setting u = ln(1 + (cos x)/3) and dv = sec(x) dx. Then du would be the derivative of ln(1 + cos(x)/3) times dx, and v would be the integral of sec(x) dx, which is ln |sec(x) + tan(x)| + C.

So, integration by parts formula is ∫ u dv = uv - ∫ v du.

Let's compute du first. The derivative of ln(1 + (cos x)/3) is [1/(1 + (cos x)/3)] * (-sin x)/3. So:

du = [ -sin x / (3 + cos x) ] dx.

And dv = sec(x) dx, so v = ln |sec(x) + tan(x)|. Since we're integrating from 0 to π, and sec(x) + tan(x) is positive in (0, π/2) and negative in (π/2, π), but the absolute value would handle that. However, at x = π/2, sec(x) is undefined, so we need to check if the integral is convergent there. But let's proceed and see.

So, applying integration by parts:

uv evaluated from 0 to π minus ∫₀^π v du.

So, first term: [ln(1 + (cos x)/3) * ln(sec x + tan x)] from 0 to π.

Let's evaluate the boundary terms. At x = π: cos(π) = -1, so 1 + (-1)/3 = 2/3. So ln(2/3). And sec(π) = -1, tan(π) = 0. So sec(π) + tan(π) = -1 + 0 = -1. The ln(-1) is problematic because logarithm of a negative number is not real. Wait, but in the original integral, sec(x) is 1/cos(x), which at x=π is -1, and ln(1 + cos(x)/3) is ln(2/3), which is real. But when we do integration by parts, the term v is ln(sec x + tan x), which at x=π is ln(-1), which is not real. That suggests that maybe integration by parts isn't the right approach here, or perhaps we need to handle the principal value or something. Hmm, this is a problem. Maybe the integral is improper at x=π/2 where sec(x) is undefined. Wait, but the original integral has sec(x) which is 1/cos(x), so at x=π/2, cos(x) is zero, so sec(x) is undefined. Therefore, the integral is improper at x=π/2. So we need to check if the integral converges there. Let's see near x=π/2, cos(x) ≈ -(x - π/2) (since cos(π/2 + h) ≈ -h for small h). So sec(x) ≈ -1/(x - π/2). The logarithm term at x near π/2: 1 + cos(x)/3 ≈ 1 + (- (x - π/2))/3. So ln(1 - (x - π/2)/3) ≈ - (x - π/2)/3. Therefore, the integrand near π/2 is approximately (-1/(x - π/2)) * (- (x - π/2)/3) = 1/3. So the integrand approaches 1/3 as x approaches π/2 from either side. Therefore, the function is actually continuous at x=π/2 in the limit, so the integral is convergent. So even though sec(x) has a singularity there, the logarithm term cancels it out. Therefore, the integral is proper. So maybe the integration by parts is still possible, but the boundary term at x=π is problematic because ln(-1) is not real. But the original integral is real, so perhaps the imaginary parts cancel out? Wait, but the original integral is real, so maybe the boundary terms end up being real. Let's check the boundary terms more carefully.

At x=π: ln(1 + cos(π)/3) = ln(1 - 1/3) = ln(2/3). And ln(sec(π) + tan(π)) = ln(-1 + 0) = ln(-1) = iπ (principal value). So the term would be ln(2/3) * iπ. Similarly, at x=0: ln(1 + cos(0)/3) = ln(1 + 1/3) = ln(4/3). And ln(sec(0) + tan(0)) = ln(1 + 0) = ln(1) = 0. So the boundary term is [ln(2/3) * iπ - ln(4/3) * 0] = iπ ln(2/3). But the original integral is real, so this suggests that the remaining integral (the ∫ v du part) must cancel out the imaginary part. But this seems complicated. Maybe integration by parts is not the right approach here. Let me think of another method.

Alternatively, perhaps expanding the logarithm into a Taylor series. Let's consider the term ln(1 + (cos x)/3). The Taylor series for ln(1 + y) is Σ_{n=1}^∞ (-1)^{n+1} y^n / n for |y| < 1. Here, y = cos x /3. Since |cos x| ≤ 1, so |y| ≤ 1/3 < 1, so the series converges for all x. Therefore, we can write:

ln(1 + cos x /3) = Σ_{n=1}^∞ (-1)^{n+1} (cos x)^n / (3^n n).

Then, multiplying by sec x, which is 1/cos x, so the integrand becomes:

Σ_{n=1}^∞ (-1)^{n+1} (cos x)^{n -1} / (3^n n).

Therefore, the integral becomes:

∫₀^π Σ_{n=1}^∞ (-1)^{n+1} (cos x)^{n -1} / (3^n n) dx.

If we can interchange the integral and the summation, then we can compute each term individually. Let's check if that's possible. Since the series converges uniformly on [0, π], by the Weierstrass M-test: |(-1)^{n+1} (cos x)^{n -1} / (3^n n)| ≤ (1)^{n -1} / (3^n n) = 1/(3^n n), and Σ 1/(3^n n) converges (since it's a convergent series). Therefore, we can interchange the integral and the summation.

Therefore, the integral becomes:

Σ_{n=1}^∞ [ (-1)^{n+1} / (3^n n) ∫₀^π (cos x)^{n -1} dx ].

So, let's denote I_n = ∫₀^π (cos x)^{n -1} dx. Then, the integral is the sum over n of (-1)^{n+1} I_n 3^{-n} / n.

So, we need to compute I_n for n ≥1. Let's note that (cos x)^{k} can be integrated over 0 to π using standard integrals. For integer k, the integral ∫₀^π cos^k x dx is known. Specifically, for even and odd exponents.

Recall that ∫₀^π cos^{m}x dx = 2 ∫₀^{π/2} cos^{m}x dx when m is even, and 0 when m is odd. Wait, no. Wait, for even m, cos^m x is symmetric around π/2, so the integral from 0 to π is twice the integral from 0 to π/2. For odd m, the integral from 0 to π is zero because the positive and negative areas cancel out. Wait, but cos(x) from 0 to π is symmetric around π/2, but for even exponents, it's positive on both sides, and for odd exponents, it's positive on [0, π/2) and negative on (π/2, π]. Therefore, ∫₀^π} cos^{2k}x dx = 2 ∫₀^{π/2} cos^{2k}x dx, and ∫₀^π} cos^{2k+1}x dx = 0.

But in our case, the exponent is n -1. So, depending on whether n -1 is even or odd. Let's write n -1 = m. So, m = n -1. Then, if m is even (i.e., n is odd), then the integral is 2 ∫₀^{π/2} cos^{m}x dx. If m is odd (i.e., n is even), then the integral is 0. Therefore, I_n = ∫₀^π cos^{n -1}x dx is equal to 2 ∫₀^{π/2} cos^{n -1}x dx when n -1 is even (i.e., n is odd), and 0 when n is even.

Therefore, in our summation, only the terms with odd n contribute. Let's write n = 2k +1, where k starts from 0. Then, n =1,3,5,... So, substituting n =2k +1, then:

Sum becomes Σ_{k=0}^∞ [ (-1)^{2k +2} / (3^{2k +1} (2k +1)) * I_{2k +1} }.

But (-1)^{2k +2} = (-1)^{2k} * (-1)^2 = (1)^k *1 =1. So, the sign is always positive. Therefore, the sum simplifies to:

Σ_{k=0}^∞ [ 1 / (3^{2k +1} (2k +1)) * I_{2k +1} }.

But I_{2k +1} = ∫₀^π cos^{2k}x dx = 2 ∫₀^{π/2} cos^{2k}x dx. The integral ∫₀^{π/2} cos^{2k}x dx is known as the beta function or using the formula for even powers:

∫₀^{π/2} cos^{2k}x dx = (π/2) ( (2k)! ) / (4^k (k!)^2 ) ).

Therefore, I_{2k +1} = 2 * (π/2) ( (2k)! ) / (4^k (k!)^2 ) ) = π (2k)! / (4^k (k!)^2 ).

Therefore, substituting back into the sum:

Σ_{k=0}^∞ [ 1 / (3^{2k +1} (2k +1)) * π (2k)! / (4^k (k!)^2 ) ) ].

Simplify the terms:

3^{2k +1} = 3 * 9^k, and 4^k = (2^2)^k = 2^{2k}. So:

= π /3 Σ_{k=0}^∞ [ (2k)! / ( (9/4)^k (k!)^2 ) ) * 1/(2k +1) ) ].

Wait, let's see:

The term inside the sum is:

(2k)! / (4^k (k!)^2 ) * 1/(3^{2k +1} (2k +1)) )

Wait, no. Let me re-express:

We have:

1/(3^{2k +1}) = 1/(3 * 9^k )

and 1/(4^k) = 1/(4^k )

So combining denominators:

3^{2k +1} *4^k = 3 * (9*4)^k = 3 * 36^k

Wait, 9*4=36. So:

So, the term becomes:

π /3 * Σ_{k=0}^∞ [ (2k)! / ( (36)^k (k!)^2 ) ) * 1/(2k +1) ) ].

Hmm, this seems complicated. Maybe there's a known series for this. Let's recall that the generating function for the central binomial coefficients. The central binomial coefficient is (2k)! / (k!)^2 = C(2k, k). So, the term is C(2k, k) / (36^k (2k +1)).

So, the sum is Σ_{k=0}^∞ [ C(2k, k) / ( (36)^k (2k +1) ) ) ].

Hmm, does this series have a closed-form expression? Let me think. The generating function for C(2k, k) x^k is 1/√(1 -4x). But here we have an extra 1/(2k +1) term. Let's recall that ∫₀^1 x^{2k} dx = 1/(2k +1). So, perhaps we can write the sum as Σ_{k=0}^∞ C(2k, k) / 36^k ∫₀^1 x^{2k} dx = ∫₀^1 Σ_{k=0}^∞ C(2k, k) (x^2 /36)^k dx. Wait, x^{2k} is x^{2k}, so (x^2 /36)^k. Therefore, the sum inside is Σ_{k=0}^∞ C(2k, k) (x² /36)^k = 1/√(1 -4*(x² /36)) ) = 1/√(1 - x² /9) = 1/√( (9 -x²)/9 ) = 3 / √(9 -x²).

Therefore, the integral becomes ∫₀^1 3 / √(9 -x²) dx. Therefore, the sum is ∫₀^1 3 / √(9 -x²) dx. Let's compute that integral:

∫₀^1 3 / √(9 -x²) dx = 3 ∫₀^1 1 / √(9 -x²) dx.

The integral of 1/√(a² -x²) dx is arcsin(x/a) + C. So here, a=3, so:

3 [ arcsin(x/3) ] from 0 to1 = 3 ( arcsin(1/3) - arcsin(0) ) = 3 arcsin(1/3).

Therefore, the sum Σ_{k=0}^∞ [ C(2k, k) / (36^k (2k +1) ) ] = 3 arcsin(1/3).

Therefore, going back to the original expression:

The integral is π/3 * 3 arcsin(1/3) = π arcsin(1/3).

Wait, that's a nice simplification! So, putting it all together:

The original integral is equal to π arcsin(1/3).

But wait, let's check the steps again to make sure.

We had:

Integral = π /3 * Σ_{k=0}^∞ [ C(2k, k) / (36^k (2k +1) ) ] = π /3 * 3 arcsin(1/3) = π arcsin(1/3).

Yes, that seems right. So the integral evaluates to π times arcsin(1/3). Alternatively, since arcsin(1/3) is equal to arctan(1/√(9 -1)) = arctan(1/√8) = arctan(1/(2√2)), but maybe that's not necessary. So the exact answer is π arcsin(1/3).

But let's verify this result. Let me check with approximate numerical integration. Let's compute the integral numerically and see if it matches π arcsin(1/3).

First, compute π arcsin(1/3). Let's compute arcsin(1/3) in radians. 1/3 is approximately 0.3333. The arcsin of that is approximately 0.3398 radians. Then multiply by π: 0.3398 * 3.1416 ≈ 1.067. So the numerical value is approximately 1.067.

Alternatively, let's compute the integral numerically. Let's use a calculator or approximate method. But since I can't compute it here, but I can recall that if the analytical result is π arcsin(1/3), then the numerical value should be π * arcsin(1/3). Let's compute that more accurately.

First, compute arcsin(1/3):

Using a calculator, arcsin(1/3) ≈ 0.3398369094541219 radians.

Multiply by π: 0.3398369094541219 * π ≈ 0.3398369094541219 * 3.141592653589793 ≈ 1.0673775373657294.

Rounded to 10 decimal places, that's approximately 1.0673775374.

But let's check if this matches the actual integral. Let's consider integrating sec(x) ln(1 + cos(x)/3) from 0 to π. However, integrating through the singularity at π/2. But since the integrand is continuous there (as we saw earlier), we can compute it numerically. But since I can't do that here, but if the analytical steps are correct, then the answer should be π arcsin(1/3). Let me check if there's another way to verify.

Alternatively, perhaps differentiating the result. Let's suppose F(x) is the antiderivative. Then, F(π) - F(0) should be the integral. But since we used series expansion and term-wise integration, and arrived at π arcsin(1/3), which seems plausible.

Alternatively, let's consider a substitution. Let me try substituting t = sin x. Wait, but maybe another substitution. Let me think. Let's set y = 1 + cos x /3. Then, dy/dx = -sin x /3. But the integrand is sec x ln y. Hmm, not sure. Alternatively, perhaps a substitution related to the arcsin function.

Wait, given that the result is π arcsin(1/3), maybe there's a substitution that leads directly to that. Let me think. Let me consider the substitution θ = arcsin( (1 + cos x)/3 ). Wait, not sure. Alternatively, perhaps using a substitution t = sin x. Let's try.

Let me set t = sin x. Then, dt = cos x dx. But the integrand is sec x ln(1 + cos x /3) dx = (1/cos x) ln(1 + cos x /3) dx. So, if t = sin x, then cos x = sqrt(1 - t²), but this might complicate things. Alternatively, set u = cos x. Then, du = -sin x dx. But the integrand is (1/u) ln(1 + u/3) * (-du / sin x). But sin x = sqrt(1 - u²). So, the integral becomes:

∫_{u=1}^{u=-1} (1/u) ln(1 + u/3) * (-du) / sqrt(1 - u²) )

= ∫_{-1}^1 (1/u) ln(1 + u/3) / sqrt(1 - u²) du.

But this seems more complicated. Alternatively, split the integral into two parts: from 0 to π/2 and π/2 to π. But in the substitution, maybe symmetry can help. However, I don't see an obvious path here. Given that the series approach led us to π arcsin(1/3), and the steps seem correct, perhaps that's the right answer.

Therefore, the exact answer is π arcsin(1/3), and the numerical approximation is approximately 1.0673775374.

But let me check if there's a different form. Since arcsin(1/3) can also be expressed in terms of other inverse trigonometric functions. For example, arcsin(1/3) = arctan(1/√(9 -1)) = arctan(1/(2√2)), but that might not simplify it further. So π arcsin(1/3) is probably the simplest exact form.

Therefore, the final answer is π arcsin(1/3), and the numerical value is approximately 1.0673775374.
</think>

{"answer": "\\pi \\arcsin\\left(\\frac{1}{3}\\right)", "numerical_answer": "1.0673775374"}