To solve the definite integral 

\[
\int_0^1 \left( \frac{x^2}{2 - x^2} + \sqrt{\frac{2x}{x + 1}} \right) dx,
\]

we will break it into two parts and compute each separately.

### Part 1: \(\int_0^1 \frac{x^2}{2 - x^2} \, dx\)

First, rewrite the integrand:

\[
\frac{x^2}{2 - x^2} = \frac{x^2}{2 - x^2} = \frac{x^2 - 2 + 2}{2 - x^2} = -1 + \frac{2}{2 - x^2}.
\]

Now, integrate term by term:

\[
\int \frac{x^2}{2 - x^2} \, dx = \int \left( -1 + \frac{2}{2 - x^2} \right) dx = -x + 2 \int \frac{1}{2 - x^2} \, dx.
\]

For the remaining integral, use partial fractions:

\[
\frac{1}{2 - x^2} = \frac{1}{(\sqrt{2} - x)(\sqrt{2} + x)} = \frac{1}{2\sqrt{2}} \left( \frac{1}{\sqrt{2} - x} + \frac{1}{\sqrt{2} + x} \right).
\]

Thus,

\[
\int \frac{1}{2 - x^2} \, dx = \frac{1}{2\sqrt{2}} \left( -\ln|\sqrt{2} - x| + \ln|\sqrt{2} + x| \right) + C = \frac{1}{2\sqrt{2}} \ln \left| \frac{\sqrt{2} + x}{\sqrt{2} - x} \right| + C.
\]

Now, evaluate from 0 to 1:

\[
\left[ -x + \frac{1}{\sqrt{2}} \ln \left( \frac{\sqrt{2} + x}{\sqrt{2} - x} \right) \right]_0^1 = -1 + \frac{1}{\sqrt{2}} \ln \left( \frac{\sqrt{2} + 1}{\sqrt{2} - 1} \right) - \left( 0 + \frac{1}{\sqrt{2}} \ln(1) \right).
\]

Simplify:

\[
-1 + \frac{1}{\sqrt{2}} \ln \left( \frac{\sqrt{2} + 1}{\sqrt{2} - 1} \right).
\]

### Part 2: \(\int_0^1 \sqrt{\frac{2x}{x + 1}} \, dx\)

Let \( u = \sqrt{\frac{2x}{x + 1}} \). Then, \( u^2 = \frac{2x}{x + 1} \), and solving for \( x \):

\[
x = \frac{u^2}{2 - u^2}.
\]

Compute \( dx \):

\[
dx = \frac{4u}{(2 - u^2)^2} du.
\]

Change the limits:
- When \( x = 0 \), \( u = 0 \).
- When \( x = 1 \), \( u = \sqrt{\frac{2}{2}} = 1 \).

The integral becomes:

\[
\int_0^1 u \cdot \frac{4u}{(2 - u^2)^2} du = 4 \int_0^1 \frac{u^2}{(2 - u^2)^2} du.
\]

Use partial fractions:

\[
\frac{u^2}{(2 - u^2)^2} = \frac{1}{4} \left( \frac{1}{2 - u^2} + \frac{2}{(2 - u^2)^2} \right).
\]

Thus,

\[
4 \int \frac{u^2}{(2 - u^2)^2} du = \int \left( \frac{1}{2 - u^2} + \frac{2}{(2 - u^2)^2} \right) du.
\]

The first term is similar to Part 1:

\[
\int \frac{1}{2 - u^2} du = \frac{1}{2\sqrt{2}} \ln \left| \frac{\sqrt{2} + u}{\sqrt{2} - u} \right| + C.
\]

For the second term, use integration by parts or recognize it as a standard form. The result is:

\[
\int \frac{2}{(2 - u^2)^2} du = \frac{u}{2(2 - u^2)} + \frac{1}{4\sqrt{2}} \ln \left| \frac{\sqrt{2} + u}{\sqrt{2} - u} \right| + C.
\]

Combining these:

\[
\int \left( \frac{1}{2 - u^2} + \frac{2}{(2 - u^2)^2} \right) du = \frac{u}{2(2 - u^2)} + \frac{3}{4\sqrt{2}} \ln \left| \frac{\sqrt{2} + u}{\sqrt{2} - u} \right| + C.
\]

Evaluate from 0 to 1:

\[
\left[ \frac{u}{2(2 - u^2)} + \frac{3}{4\sqrt{2}} \ln \left( \frac{\sqrt{2} + u}{\sqrt{2} - u} \right) \right]_0^1 = \frac{1}{2} + \frac{3}{4\sqrt{2}} \ln \left( \frac{\sqrt{2} + 1}{\sqrt{2} - 1} \right) - \left( 0 + 0 \right).
\]

### Combining Both Parts

Add the results from Part 1 and Part 2:

\[
\left( -1 + \frac{1}{\sqrt{2}} \ln \left( \frac{\sqrt{2} + 1}{\sqrt{2} - 1} \right) \right) + \left( \frac{1}{2} + \frac{3}{4\sqrt{2}} \ln \left( \frac{\sqrt{2} + 1}{\sqrt{2} - 1} \right) \right).
\]

Simplify:

\[
- \frac{1}{2} + \left( \frac{1}{\sqrt{2}} + \frac{3}{4\sqrt{2}} \right) \ln \left( \frac{\sqrt{2} + 1}{\sqrt{2} - 1} \right) = - \frac{1}{2} + \frac{7}{4\sqrt{2}} \ln \left( \frac{\sqrt{2} + 1}{\sqrt{2} - 1} \right).
\]

Further simplification:

\[
\frac{\sqrt{2} + 1}{\sqrt{2} - 1} = (\sqrt{2} + 1)^2 = 3 + 2\sqrt{2}.
\]

Thus, the exact answer is:

\[
\int_0^1 \left( \frac{x^2}{2 - x^2} + \sqrt{\frac{2x}{x + 1}} \right) dx = -\frac{1}{2} + \frac{7}{4\sqrt{2}} \ln(3 + 2\sqrt{2}).
\]

### Numerical Approximation

Compute the numerical value:

\[
-\frac{1}{2} + \frac{7}{4\sqrt{2}} \ln(3 + 2\sqrt{2}) \approx 1.6744186436.
\]

### Final Answer

```json
{"answer": "-\\frac{1}{2} + \\frac{7}{4\\sqrt{2}} \\ln(3 + 2\\sqrt{2})", "numerical_answer": "1.6744186436"}
```