<think>
Okay, so I need to compute the definite integral from 0 to 1 of x³ arccos(x) arcsin²(x) dx. Hmm, that looks a bit complicated. Let me start by recalling some integration techniques. The integrand has three functions multiplied together: x³, arccos(x), and arcsin squared. That's a lot. Maybe integration by parts could work here, but with three functions, it's not straightforward. Wait, maybe I can simplify the expression first.

I know that arccos(x) and arcsin(x) are related. Specifically, arccos(x) = π/2 - arcsin(x). Maybe substituting that in could help. Let me try that. So replacing arccos(x) with π/2 - arcsin(x), the integral becomes:

∫₀¹ x³ (π/2 - arcsin(x)) (arcsin²x) dx

Expanding that, it would split into two integrals:

π/2 ∫₀¹ x³ arcsin²x dx - ∫₀¹ x³ arcsin³x dx

So now I have two integrals to compute: one with arcsin squared and another with arcsin cubed. Let me tackle them one by one. Let's start with the first one: ∫ x³ arcsin²x dx. Maybe substitution? Let me set t = arcsin(x). Then x = sin(t), and dx = cos(t) dt. Also, when x is from 0 to 1, t goes from 0 to π/2. So substituting, the integral becomes:

∫₀^{π/2} (sin³t) t² cos(t) dt

Simplify sin³t cos(t). Let's note that sin³t cos(t) is sin³t * cos t. Maybe we can write sin³t as sin²t * sint, so sin²t = 1 - cos²t. So:

sin³t cos t = (1 - cos²t) sint cos t

But maybe substitution u = sin t? Then du = cos t dt. Wait, but we have t² in there as well. Hmm, this might get complicated. Alternatively, perhaps integration by parts. Let me consider integrating by parts for ∫ t² sin³t cos t dt. Wait, but the integrand is t² sin³t cos t. Let me first simplify sin³t cos t. Let's see, sin³t cos t can be written as sin^3 t cos t. Let me note that the derivative of sin^4 t is 4 sin^3 t cos t. So maybe that's a useful observation. Let me check:

d/dt [sin^4 t] = 4 sin^3 t cos t. So sin^3 t cos t = (1/4) d/dt [sin^4 t]. Therefore, the integral becomes:

∫ t² * (1/4) d/dt [sin^4 t] dt

So integrating by parts, let me set u = t² and dv = (1/4) d/dt [sin^4 t] dt. Then du = 2t dt, and v = (1/4) sin^4 t. So integration by parts formula is uv| - ∫ v du. So:

(1/4) t² sin^4 t | from 0 to π/2 - (1/4) ∫ sin^4 t * 2t dt

Evaluate the first term at the limits. At π/2, sin(π/2) = 1, so sin^4(π/2) = 1, so term is (1/4)(π/2)^2 * 1 = (1/4)(π²/4) = π²/16. At 0, sin(0) = 0, so that term is 0. So the first part is π²/16. Then the remaining integral is - (1/4)*2 ∫ t sin^4 t dt = - (1/2) ∫ t sin^4 t dt.

So now we have:

π²/16 - (1/2) ∫ t sin^4 t dt

Now, need to compute ∫ t sin^4 t dt. Hmm, this seems recursive. Let's see. Maybe another integration by parts. Let me set u = t, dv = sin^4 t dt. Then du = dt, and v = ∫ sin^4 t dt. But integrating sin^4 t is a standard integral. Let me recall that sin^4 t can be written using power-reduction formulas. For example, sin^4 t = (3/8) - (1/2) cos(2t) + (1/8) cos(4t). Wait, let me compute that.

Using the identity: sin^4 t = (1 - cos 2t)/2 squared. So:

sin^2 t = (1 - cos 2t)/2, so sin^4 t = [(1 - cos 2t)/2]^2 = (1 - 2 cos 2t + cos²2t)/4. Then, cos²2t can be written as (1 + cos 4t)/2. So:

sin^4 t = [1 - 2 cos 2t + (1 + cos 4t)/2]/4 = [2 - 4 cos 2t + 1 + cos 4t]/8 = [3 - 4 cos 2t + cos 4t]/8. So:

sin^4 t = 3/8 - (1/2) cos 2t + (1/8) cos 4t.

Therefore, integrating sin^4 t dt:

∫ sin^4 t dt = 3/8 t - (1/2)(1/2) sin 2t + (1/8)(1/4) sin 4t + C = 3t/8 - (1/4) sin 2t + (1/32) sin 4t + C.

So v = ∫ sin^4 t dt = 3t/8 - (1/4) sin 2t + (1/32) sin 4t + C. So going back to integration by parts:

∫ t sin^4 t dt = u v - ∫ v du = t [3t/8 - (1/4) sin 2t + (1/32) sin 4t] - ∫ [3t/8 - (1/4) sin 2t + (1/32) sin 4t] dt

Let's compute this term by term.

First term: t*(3t/8 - (1/4) sin 2t + (1/32) sin 4t) evaluated from 0 to π/2. Then subtract the integral of [3t/8 - (1/4) sin 2t + (1/32) sin 4t] dt.

Let me compute the first part:

At t = π/2: (π/2)*(3*(π/2)/8 - (1/4) sin π + (1/32) sin 2π) = (π/2)*(3π/16 - 0 + 0) = (π/2)*(3π/16) = 3π²/32.

At t = 0: 0*(...) = 0. So the first part is 3π²/32.

Now, the integral to subtract is:

∫ [3t/8 - (1/4) sin 2t + (1/32) sin 4t] dt

Integrate term by term:

∫ 3t/8 dt = (3/16) t²

∫ -(1/4) sin 2t dt = (1/8) cos 2t

∫ (1/32) sin 4t dt = -(1/128) cos 4t

So the integral is (3/16) t² + (1/8) cos 2t - (1/128) cos 4t evaluated from 0 to π/2.

Evaluate at π/2:

(3/16)(π²/4) + (1/8) cos π - (1/128) cos 2π

= 3π²/64 + (1/8)(-1) - (1/128)(1)

= 3π²/64 - 1/8 - 1/128

At 0:

(0) + (1/8)(1) - (1/128)(1) = 1/8 - 1/128 = 16/128 - 1/128 = 15/128

So the integral from 0 to π/2 is [3π²/64 - 1/8 - 1/128] - [15/128] = 3π²/64 - 1/8 - 1/128 -15/128 = 3π²/64 - 1/8 - 16/128 = 3π²/64 - 1/8 - 1/8 = 3π²/64 - 1/4

Therefore, the integral ∫ t sin^4 t dt is:

3π²/32 - [3π²/64 - 1/4] = 3π²/32 - 3π²/64 + 1/4 = (6π² - 3π²)/64 + 1/4 = 3π²/64 + 1/4

So going back to the previous step, the original integral for the first part was:

π²/16 - (1/2)(3π²/64 + 1/4) = π²/16 - 3π²/128 - 1/8 = (8π² - 3π²)/128 - 1/8 = 5π²/128 - 1/8

So that's the result of the first integral: π/2 ∫ x³ arcsin²x dx = 5π²/128 - 1/8

Wait, no. Wait, let me check. Wait, the first integral after substitution was:

π/2 times ∫ x³ arcsin²x dx, which after substitution became π/2 times [π²/16 - (1/2)(3π²/64 + 1/4)].

Wait, no. Wait, let's retrace. The first integral was:

Original integral after substitution: π/2 ∫₀¹ x³ arcsin²x dx = π/2 * [π²/16 - (1/2)(3π²/64 + 1/4)].

Wait, no. Wait, the first integral was ∫₀¹ x³ arcsin²x dx transformed into ∫₀^{π/2} t² sin³t cos t dt, which after integration by parts became π²/16 - (1/2)(3π²/64 + 1/4). So the value of ∫ x³ arcsin²x dx is π²/16 - (1/2)(3π²/64 + 1/4) = π²/16 - 3π²/128 - 1/8 = (8π² - 3π²)/128 - 1/8 = 5π²/128 - 1/8.

So then multiplying by π/2, we get:

π/2 * (5π²/128 - 1/8) = 5π³/256 - π/16

That's the first part. Now, the second integral is ∫₀¹ x³ arcsin³x dx. Let's tackle that.

Again, substitution t = arcsin(x), so x = sin t, dx = cos t dt, limits from 0 to π/2. So the integral becomes:

∫₀^{π/2} sin³t * t³ * cos t dt

Again, similar to before. Let's write sin³t cos t as sin³t cos t. Let me use the same approach as before. Note that sin³t cos t is (1/4) d/dt [sin^4 t]. So:

∫ t³ * (1/4) d/dt [sin^4 t] dt

Integration by parts: set u = t³, dv = (1/4) d/dt [sin^4 t] dt. Then du = 3t² dt, v = (1/4) sin^4 t.

So applying integration by parts:

(1/4) t³ sin^4 t | from 0 to π/2 - (1/4) ∫ sin^4 t * 3t² dt

Evaluating the first term: at π/2, sin^4(π/2) = 1, so (1/4)(π/2)^3 * 1 = (1/4)(π³/8) = π³/32. At 0, it's 0. So the first term is π³/32. The remaining integral is - (3/4) ∫ t² sin^4 t dt.

Wait, but we already computed ∫ t² sin^4 t dt earlier. Wait, in the first integral, we had ∫ t² sin^3 t cos t dt, which after substitution became ∫ t² sin^3 t cos t dt, which was transformed into ∫ t² sin^3 t cos t dt. Wait, no, actually, in the first integral, after substitution t = arcsin x, we had ∫ t² sin³t cos t dt, which was integrated by parts. Wait, but here, the integral is ∫ t² sin^4 t dt. Wait, no, in the first integral, after substitution, we had ∫ t² sin³t cos t dt, which was transformed into π²/16 - (1/2) ∫ t sin^4 t dt. But here, the integral is ∫ t² sin^4 t dt. So this is a different integral. Hmm, so we need to compute ∫ t² sin^4 t dt.

Wait, but maybe we can use the same approach. Let me see. Let's write sin^4 t as (3/8 - (1/2) cos 2t + (1/8) cos 4t). So:

∫ t² sin^4 t dt = ∫ t² [3/8 - (1/2) cos 2t + (1/8) cos 4t] dt = 3/8 ∫ t² dt - (1/2) ∫ t² cos 2t dt + (1/8) ∫ t² cos 4t dt

Compute each integral separately.

First integral: 3/8 ∫ t² dt from 0 to π/2 = 3/8 * [t³/3] from 0 to π/2 = 3/8 * (π³/24) = π³/64

Second integral: -(1/2) ∫ t² cos 2t dt. Let's compute ∫ t² cos 2t dt. Integration by parts. Let u = t², dv = cos 2t dt. Then du = 2t dt, v = (1/2) sin 2t. So:

uv - ∫ v du = (t²)(1/2 sin 2t) - ∫ (1/2 sin 2t)(2t dt) = (t²/2) sin 2t - ∫ t sin 2t dt

Now, compute ∫ t sin 2t dt. Again, integration by parts. Let u = t, dv = sin 2t dt. Then du = dt, v = - (1/2) cos 2t.

So:

- (1/2) t cos 2t + (1/2) ∫ cos 2t dt = - (1/2) t cos 2t + (1/4) sin 2t + C

Putting it all together:

∫ t² cos 2t dt = (t²/2) sin 2t - [ - (1/2) t cos 2t + (1/4) sin 2t ] + C = (t²/2) sin 2t + (1/2) t cos 2t - (1/4) sin 2t + C

Therefore, the second integral is:

- (1/2) [ (t²/2) sin 2t + (1/2) t cos 2t - (1/4) sin 2t ] evaluated from 0 to π/2.

Let's compute this at π/2:

First term: ( (π/2)^2 / 2 ) sin π + (1/2)(π/2) cos π - (1/4) sin π

sin π = 0, cos π = -1, so:

0 + (1/2)(π/2)(-1) - 0 = - π/4

At 0:

All terms are 0. So the value is - π/4 - 0 = - π/4

So the second integral is - (1/2)( - π/4 ) = π/8

Third integral: (1/8) ∫ t² cos 4t dt. Let's compute ∫ t² cos 4t dt. Again, integration by parts. Let u = t², dv = cos 4t dt. Then du = 2t dt, v = (1/4) sin 4t.

So:

uv - ∫ v du = (t²)(1/4 sin 4t) - ∫ (1/4 sin 4t)(2t dt) = (t²/4) sin 4t - (1/2) ∫ t sin 4t dt

Compute ∫ t sin 4t dt. Integration by parts: u = t, dv = sin 4t dt. Then du = dt, v = - (1/4) cos 4t.

So:

- (1/4) t cos 4t + (1/4) ∫ cos 4t dt = - (1/4) t cos 4t + (1/16) sin 4t + C

Therefore, ∫ t² cos 4t dt = (t²/4) sin 4t - (1/2)[ - (1/4) t cos 4t + (1/16) sin 4t ] + C = (t²/4) sin 4t + (1/8) t cos 4t - (1/32) sin 4t + C

Now, evaluate from 0 to π/2:

At π/2:

(t²/4) sin 4*(π/2) + ( (π/2)^2 /4 ) sin 2π + (1/8)(π/2) cos 2π - (1/32) sin 2π

sin 2π = 0, cos 2π = 1. So:

0 + (1/8)(π/2)(1) - 0 = π/16

At 0:

All terms are 0. So the integral from 0 to π/2 is π/16 - 0 = π/16

Therefore, the third integral is (1/8) * π/16 = π/128

Putting all three integrals:

First: π³/64

Second: π/8

Third: π/128

So ∫ t² sin^4 t dt = π³/64 + π/8 + π/128 = π³/64 + 16π/128 + π/128 = π³/64 + 17π/128

Wait, let me check:

Wait, the first integral was 3/8 ∫ t² dt = 3/8 * π³/24 = π³/64

Second integral: - (1/2) ∫ t² cos 2t dt = π/8

Third integral: (1/8) ∫ t² cos 4t dt = π/128

So total ∫ t² sin^4 t dt = π³/64 + π/8 + π/128

Convert to common denominator 128:

π³/64 = 2π³/128

π/8 = 16π/128

π/128 = π/128

So total: (2π³ + 16π + π)/128 = (2π³ + 17π)/128

Therefore, ∫ t² sin^4 t dt = (2π³ + 17π)/128

So going back to the second part, the integral ∫ t³ sin^3t cos t dt (which was transformed into ∫ t³ sin^3t cos t dt = π³/32 - (3/4) ∫ t² sin^4 t dt) becomes:

π³/32 - (3/4)*(2π³ + 17π)/128 = π³/32 - (3*(2π³ + 17π))/512 = π³/32 - (6π³ + 51π)/512

Convert π³/32 to 16π³/512:

16π³/512 - 6π³/512 - 51π/512 = (10π³ - 51π)/512

So the second integral ∫ x³ arcsin³x dx is equal to (10π³ - 51π)/512

Therefore, the original integral is:

π/2 ∫ x³ arcsin²x dx - ∫ x³ arcsin³x dx = [5π³/256 - π/16] - [(10π³ - 51π)/512]

Let me compute this:

First term: 5π³/256 - π/16

Second term: - (10π³ - 51π)/512

Convert to common denominator 512:

5π³/256 = 10π³/512

π/16 = 32π/512

So first term: 10π³/512 - 32π/512

Second term: -10π³/512 + 51π/512

Adding them together:

(10π³ - 32π -10π³ + 51π)/512 = (19π)/512

So the final result is 19π/512

Wait, that's it? Let me check the arithmetic again.

Original expression:

[5π³/256 - π/16] - [(10π³ - 51π)/512]

Convert to 512 denominator:

5π³/256 = 10π³/512

π/16 = 32π/512

So first part: 10π³/512 - 32π/512

Second part: - (10π³ - 51π)/512 = -10π³/512 + 51π/512

Now, combining:

10π³ - 32π -10π³ +51π = (10π³ -10π³) + (-32π +51π) = 19π

So total is 19π/512

So the exact answer is 19π/512. Let me check if that makes sense. Let's compute the numerical approximation. 19π/512 ≈ 19*3.1415926535 / 512 ≈ 19*3.1415926535 ≈ 59.6902604165 / 512 ≈ 0.1165825391. Let me check with a numerical approximation.

Alternatively, maybe I made a mistake in the sign. Let me verify the steps again.

Original integral: ∫₀¹ x³ arccos x arcsin²x dx = ∫₀¹ x³ (π/2 - arcsinx) arcsin²x dx = π/2 ∫ x³ arcsin²x dx - ∫ x³ arcsin³x dx

Computed ∫ x³ arcsin²x dx = 5π²/128 - 1/8

Wait, no. Wait, earlier steps:

Wait, when we computed ∫ x³ arcsin²x dx, after substitution and integration by parts, we found that ∫ x³ arcsin²x dx = π²/16 - (1/2)(3π²/64 + 1/4) = 5π²/128 - 1/8. Then multiplying by π/2 gives (5π²/128 - 1/8) * π/2 = 5π³/256 - π/16.

Then, ∫ x³ arcsin³x dx was computed as (10π³ -51π)/512. So the original integral is:

5π³/256 - π/16 - (10π³ -51π)/512

Convert to 512 denominator:

5π³/256 = 10π³/512

π/16 = 32π/512

So:

10π³/512 - 32π/512 -10π³/512 +51π/512 = (10π³ -10π³)/512 + (-32π +51π)/512 = 19π/512

Yes, that's correct. So the exact answer is 19π/512. Let me compute the numerical value:

19 * 3.141592653589793 / 512 ≈ (19 * 3.141592653589793) ≈ 59.69026041820607 / 512 ≈ 0.1165825391

So approximately 0.1165825391. Let me check with a calculator or approximate integral.

Alternatively, maybe I can use substitution to verify. But given the steps, it seems correct. So the exact answer is 19π/512, and the numerical approximation is approximately 0.1165825391.
</think>

{"answer": "\\dfrac{19\\pi}{512}", "numerical_answer": 0.1165825391}