We start with the integral

  I = ∫ from x = 1 to ∞ (x² – 1²)^(2 – 1/2) e^(–0.5² x²) H_(2×2+1)(0.5 x) dx.

Notice that
  2 – 1/2 = 3/2  and  H_(2×2+1)(0.5 x) = H₅(0.5 x).

Step 1. Write out the Hermite polynomial in closed‐form.
For the “physicists’” Hermite polynomials the fifth degree polynomial is
  H₅(z) = 32z⁵ – 160z³ + 120z.
Thus, with z = 0.5x we have
  H₅(0.5x) = 32(0.5x)⁵ – 160(0.5x)³ + 120(0.5x)
     = 32 (x⁵/32) – 160 (x³/8) + 120 (x/2)
     = x⁵ – 20x³ + 60x.

Step 2. Substitute this into the integral.
Also note that 1.0² = 1 and (x²–1)^(3/2) remains. Finally, 0.5² = 0.25 so that e^(–0.5²x²) = e^(–0.25x²).

Thus the integral becomes

  I = ∫₁∞ (x² – 1)^(3/2) e^(–0.25x²) (x⁵ – 20x³ + 60x) dx.

Step 3. Change of variable.
It is very useful to make the substitution t = x². Then
  dt/dx = 2x  or  dx = dt/(2x).
Also, note that
  x² – 1 = t – 1  and  (x²–1)^(3/2) = (t – 1)^(3/2).
We now rewrite the polynomial:
  x⁵ = t^(5/2),  x³ = t^(3/2),  x = t^(1/2).
Thus,
  x⁵ – 20x³ + 60x = t^(5/2) – 20 t^(3/2) + 60 t^(1/2).

Also, the factor dx/(2x) gives:
  dx = dt/(2√t).

Putting these in, and with the exponential becoming e^(–0.25t), we have

  I = ∫ from t=1 to ∞ (t – 1)^(3/2) e^(–0.25t) [t^(5/2) – 20t^(3/2) + 60t^(1/2)] (dt/(2√t)).

Simplify the powers of t by writing each term divided by √t:
  t^(5/2)/√t = t²,
  t^(3/2)/√t = t,
  t^(1/2)/√t = 1.

Thus the integral becomes

  I = (1/2) ∫₁∞ (t – 1)^(3/2) e^(–0.25t) [t² – 20t + 60] dt.

Step 4. Shift the integration variable.
Let u = t – 1 so that t = u + 1 and dt = du. When t = 1, u = 0 and when t → ∞, u → ∞. In addition,
  (t – 1)^(3/2) = u^(3/2)
and the exponential becomes
  e^(–0.25t) = e^(–0.25(u + 1)) = e^(–0.25u) e^(–0.25).

The polynomial becomes
  (u + 1)² – 20(u + 1) + 60 = u² + 2u + 1 – 20u – 20 + 60 = u² – 18u + 41.

Thus

  I = (e^(–0.25)/2) ∫₀∞ u^(3/2) e^(–0.25u) (u² – 18u + 41) du.

Step 5. Express the resulting integrals in terms of Gamma functions.
We now write I as a sum of three integrals:
  I = (e^(–0.25)/2) [ ∫₀∞ u^(7/2) e^(–0.25u) du – 18 ∫₀∞ u^(5/2) e^(–0.25u) du + 41 ∫₀∞ u^(3/2) e^(–0.25u) du ].
Recall the Gamma integral formula:
  ∫₀∞ u^(s–1) e^(–λu) du = Γ(s)/λ^(s).
Match exponents:
• For u^(7/2): s – 1 = 7/2 gives s = 9/2.
• For u^(5/2): s = 7/2.
• For u^(3/2): s = 5/2.
Also, here λ = 0.25.

Thus we have:
  ∫₀∞ u^(7/2) e^(–0.25u) du = Γ(9/2)/(0.25)^(9/2),
  ∫₀∞ u^(5/2) e^(–0.25u) du = Γ(7/2)/(0.25)^(7/2),
  ∫₀∞ u^(3/2) e^(–0.25u) du = Γ(5/2)/(0.25)^(5/2).

Therefore,

  I = e^(–0.25)/2 [ Γ(9/2)/(0.25)^(9/2) – 18 Γ(7/2)/(0.25)^(7/2) + 41 Γ(5/2)/(0.25)^(5/2) ].

Step 6. Simplify the factors.
Since 0.25 = 1/4, note that
  (1/4)^(s) = 4^(–s) = 2^(–2s).

Thus,
  (0.25)^(9/2) = 2^(–9),
  (0.25)^(7/2) = 2^(–7),
  (0.25)^(5/2) = 2^(–5).

Then

  I = e^(–0.25)/2 [ 2⁹ Γ(9/2) – 18·2⁷ Γ(7/2) + 41·2⁵ Γ(5/2) ].

Now, we recall the half-integer Gamma function values:
  Γ(9/2) = (7/2)(5/2)(3/2)(1/2) √π = (105 √π)/16,
  Γ(7/2) = (5/2)(3/2)(1/2) √π = (15 √π)/8,
  Γ(5/2) = (3/2)(1/2) √π = (3 √π)/4.

Substitute these into I:

First term:
  2⁹ Γ(9/2) = 512 · (105√π/16) = (512/16)·105√π = 32 · 105√π = 3360√π.

Second term:
  18·2⁷ Γ(7/2) = 18 · 128 · (15√π/8) = 18 · (128/8) · 15√π = 18 · 16 · 15√π = 4320√π.

Third term:
  41·2⁵ Γ(5/2) = 41 · 32 · (3√π/4) = 41 · (32/4) · 3√π = 41 · 8 · 3√π = 984√π.

Thus the bracket becomes:
  3360√π – 4320√π + 984√π = (3360 – 4320 + 984)√π = 24√π.

Then
  I = e^(–0.25)/2 · 24√π = 12 e^(–0.25) √π.

So the exact answer is

  I = 12 √π e^(–1/4).

Step 7. Numerical approximation.
We now compute:
  √π ≈ 1.772453850905516,
  e^(–1/4) = e^(–0.25) ≈ 0.778800783071405.
Then
  12 √π e^(–1/4) ≈ 12 × 1.772453850905516 × 0.778800783071405 ≈ 16.5786195060.

Thus the final answer is:

{"answer": "$12 \\sqrt{\\pi}e^{-1/4}$", "numerical_answer": "16.5786195060"}