# Evaluating $\int_0^1e^{e^x}-e^{e^x-x}\:dx$

I'll solve this integral by analyzing each term separately.

## Step 1: Analyze the integrand

The integrand is:
$$e^{e^x}-e^{e^x-x}$$

Let's rewrite the second term:
$$e^{e^x-x} = e^{e^x} \cdot e^{-x} = \frac{e^{e^x}}{e^x}$$

So our integrand becomes:
$$e^{e^x}-\frac{e^{e^x}}{e^x} = e^{e^x} - \frac{e^{e^x}}{e^x} = e^{e^x}\left(1-\frac{1}{e^x}\right) = e^{e^x}\left(1-e^{-x}\right)$$

## Step 2: Substitute and simplify

Let's substitute $u = e^x$. Then:
- $x = \ln u$
- $dx = \frac{1}{u}du$
- When $x = 0$, $u = e^0 = 1$
- When $x = 1$, $u = e^1 = e$

Our integral becomes:
$$\int_0^1 e^{e^x}\left(1-e^{-x}\right) dx = \int_1^e e^u \left(1-\frac{1}{u}\right) \frac{1}{u}du = \int_1^e \frac{e^u}{u}\left(1-\frac{1}{u}\right)du$$

Simplifying further:
$$\int_1^e \frac{e^u}{u}\left(1-\frac{1}{u}\right)du = \int_1^e \frac{e^u}{u}du - \int_1^e \frac{e^u}{u^2}du$$

## Step 3: Evaluate the first part

For the first part $\int_1^e \frac{e^u}{u}du$, we can use the special function called the exponential integral $\text{Ei}(u) = \int \frac{e^u}{u}du$.

$$\int_1^e \frac{e^u}{u}du = \text{Ei}(e) - \text{Ei}(1)$$

## Step 4: Evaluate the second part

For the second part $\int_1^e \frac{e^u}{u^2}du$, we can use integration by parts.

Let $v = \frac{1}{u}$ and $dw = e^u du$. Then $dv = -\frac{1}{u^2}du$ and $w = e^u$.

$$\int \frac{e^u}{u^2}du = -\int e^u \cdot \frac{1}{u^2}du = -\frac{e^u}{u} + \int \frac{e^u}{u}du$$

So:
$$\int_1^e \frac{e^u}{u^2}du = \left[-\frac{e^u}{u}\right]_1^e + \int_1^e \frac{e^u}{u}du$$

$$= -\frac{e^e}{e} + \frac{e^1}{1} + \text{Ei}(e) - \text{Ei}(1)$$

$$= -1 + e + \text{Ei}(e) - \text{Ei}(1)$$

## Step 5: Combine the results

Now, going back to our original expression:
$$\int_1^e \frac{e^u}{u}du - \int_1^e \frac{e^u}{u^2}du$$

$$= \text{Ei}(e) - \text{Ei}(1) - (-1 + e + \text{Ei}(e) - \text{Ei}(1))$$

$$= \text{Ei}(e) - \text{Ei}(1) + 1 - e - \text{Ei}(e) + \text{Ei}(1)$$

$$= 1 - e$$

## Step 6: Final result

The definite integral is:
$$\int_0^1 e^{e^x}-e^{e^x-x} dx = 1 - e$$

## Numerical approximation

The value of $1 - e$ is approximately $1 - 2.71828...$ = $-1.71828...$

Calculating to 10 decimal places: $1 - e \approx -1.7182818285$

{"answer": "1-e", "numerical_answer": "-1.7182818285"}