Let \( f(x) = \lfloor \log_{2023} x \rfloor \) and consider the definite integral:
\[
I = \int_0^1 \lfloor \log_{2023} x \rfloor \, dx
\]

**Step 1: Understanding the behavior of \( \lfloor \log_{2023} x \rfloor \) on \((0,1)\)**
- For \(x \in (0,1)\), \(\log_{2023} x < 0\), so the floor is a negative integer, possibly tending to \(-\infty\) as \(x\to 0^+\).
- For any integer \(n \leq -1\), on the interval \(x \in [2023^{n}, 2023^{n+1})\), we have \(\log_{2023} x \in [n, n+1)\), so \(\lfloor \log_{2023} x \rfloor = n\).

**The intervals of constancy are:**
\[
x \in [2023^n, 2023^{n+1}), \quad n = -1, -2, -3, \dots
\]
with \(2023^n \geq 0\) for all \(n\) (since \(2023>1\)), and
\(2023^0 = 1\), \(2023^{-1} = 1/2023\), \(2023^{-2} = 1/2023^2\), etc.

So as \(x\) goes from 0 to 1, the function \(\lfloor \log_{2023} x \rfloor\) takes all negative integer values, with
\(x \in [2023^{n}, 2023^{n+1})\) being mapped to \(n\), for \(n = -1, -2, -3, \dots\)

**Step 2: Express the integral as a sum over these intervals**

Note that for \(0 < x < 1\),
\[
\bigcup_{n=-\infty}^{-1} [2023^n, 2023^{n+1}) = (0, 1)
\]
\[
I = \int_0^1 \lfloor \log_{2023} x \rfloor \, dx = \sum_{n=-\infty}^{-1} \int_{2023^n}^{2023^{n+1}} n \, dx
\]
\[
= \sum_{n=-\infty}^{-1} n \left(2023^{n+1} - 2023^n\right)
\]

Let’s reindex the sum to make it more convenient.
Let’s let \(k = -n\), so that when \(n = -1\), \(k = 1\), \(n = -2\), \(k = 2\), etc., and as \(n \to -\infty\), \(k \to \infty\).

So:
\[
n = -k, \quad k = 1,2,\ldots
\]
\[
I = \sum_{k=1}^\infty (-k) (2023^{-k+1} - 2023^{-k})
\]
Let’s factor \(2023^{-k}\):
\[
2023^{-k+1} = 2023 \cdot 2023^{-k} = 2023^{-k} \cdot 2023
\]
So
\[
I = \sum_{k=1}^\infty \left[-k(2023 \cdot 2023^{-k} - 2023^{-k})\right]
= \sum_{k=1}^\infty -k(2023-1) 2023^{-k}
= - (2023-1) \sum_{k=1}^\infty k 2023^{-k}
\]
\[
I = -2022 \sum_{k=1}^\infty k \cdot 2023^{-k}
\]

**Now**: Compute the sum \(S = \sum_{k=1}^\infty k r^k\) with \(r = 2023^{-1}\).

Recall that:
\[
\sum_{k=1}^\infty k r^k = \frac{r}{(1 - r)^2} \quad \text{for } |r| < 1
\]
Here, \(r = 1/2023 < 1\).

So,
\[
I = -2022 \cdot \frac{\frac{1}{2023}}{(1 - \frac{1}{2023})^2}
\]
\[
1 - \frac{1}{2023} = \frac{2023 - 1}{2023} = \frac{2022}{2023}
\]
Thus,
\[
I = -2022 \cdot \frac{1/2023}{(2022/2023)^2}
= -2022 \cdot \frac{1/2023}{2022^2 / 2023^2}
= -2022 \cdot \frac{1}{2023} \cdot \frac{2023^2}{2022^2}
= -2022 \cdot \frac{2023^2}{2023 \cdot 2022^2}
= -2022 \cdot \frac{2023}{2022^2}
= -\frac{2022 \cdot 2023}{2022^2}
= -\frac{2023}{2022}
\]

**Final analytic answer:**
\[
\boxed{I = -\frac{2023}{2022}}
\]

**Step 3: Numerical approximation**

Compute \(-\frac{2023}{2022}\) to 10 decimal places:

\[
\frac{2023}{2022} = 1.000494559 \text{ (to 9 decimal places, let's check more)}
\]
Let's compute it:
\(2023 \div 2022 = 1 + 1/2022 = 1 + 0.000494559\)
So,
\[
\frac{1}{2022} \approx 0.000494558997
\]
So,
\[
\frac{2023}{2022} = 1.00049455899703 \ldots
\]

Therefore,
\[
-\frac{2023}{2022} \approx -1.0004945590
\]
(Rounded to 10 decimal places)

**Step 4: Final JSON output**
```json
{"answer": "-\\frac{2023}{2022}", "numerical_answer": "-1.0004945590"}
```