We start with the integral

  I = ∫₀² x^(1/2) (2 – x)^(–1/2) cos(√(x(2 – x))) dx.

Step 1. Substitution

Let
  x = 2 sin²θ,
so that when x = 0, θ = 0 and when x = 2, sin²θ = 1 so that θ = π/2.
Differentiate:
  dx = 4 sinθ cosθ dθ.
Also,
  √x = √(2 sin²θ) = √2 sinθ,
and
  (2 – x)^(–1/2) = (2 – 2 sin²θ)^(–1/2) = [2 cos²θ]^(–1/2) = 1/(√2 cosθ).

The factor x^(1/2)(2 – x)^(–1/2) becomes
  (√2 sinθ)/(√2 cosθ) = tanθ.

Next, we compute
  √(x(2 – x)) = √[(2 sin²θ)(2 cos²θ)] = √(4 sin²θ cos²θ) = 2 sinθ cosθ.
Thus, cos(√(x(2 – x))) = cos(2 sinθ cosθ).

Then the integrand and dx combine as follows:
  x^(1/2)(2 – x)^(–1/2) cos(√(x(2 – x))) dx
    = tanθ · cos(2 sinθ cosθ) · [4 sinθ cosθ dθ]
    = 4 sinθ cosθ (tanθ) cos(2 sinθ cosθ) dθ.
Since tanθ = sinθ/cosθ, we have
  4 sinθ cosθ (sinθ/cosθ) = 4 sin²θ.
Thus, the integral becomes

  I = 4 ∫₀^(π/2) sin²θ cos(2 sinθ cosθ) dθ.

Step 2. Rewrite in “double‐angle” form

Recall the double‐angle identity:
  sin2θ = 2 sinθ cosθ.
Thus,
  2 sinθ cosθ = sin2θ,
so that cos(2 sinθ cosθ) = cos(sin2θ).

Then
  I = 4 ∫₀^(π/2) sin²θ cos(sin2θ) dθ.

Express sin²θ using the double-angle formula:
  sin²θ = (1 – cos2θ)/2.
Thus,
  I = 4 ∫₀^(π/2) (1 – cos2θ)/2 · cos(sin2θ) dθ = 2 ∫₀^(π/2) (1 – cos2θ) cos(sin2θ) dθ.

Now perform the substitution
  φ = 2θ  ⇒ dφ = 2 dθ  ⇒ dθ = dφ/2.
When θ goes from 0 to π/2, φ goes from 0 to π. Substituting gives

  I = 2 ∫₀^π (1 – cosφ) cos(sinφ) (dφ/2) = ∫₀^π (1 – cosφ) cos(sinφ) dφ.

Step 3. Express the result in closed‐form

We split the last integral into two parts:

  I = ∫₀^π cos(sinφ) dφ – ∫₀^π cosφ cos(sinφ) dφ.

It is known (see, e.g., integral representations of Bessel functions) that
  ∫₀^π cos(z sinφ) dφ = π J₀(z),
and with z = 1 we have
  ∫₀^π cos(sinφ) dφ = π J₀(1).

Next, note that the Fourier expansion of cos(sinφ) reads
  cos(sinφ) = J₀(1) + 2 ∑ₙ₌₁^∞ J₂ₙ(1) cos(2nφ).
Since there is no cosφ term in this expansion (only even multiples of φ appear), it follows from orthogonality that
  ∫₀^π cosφ cos(sinφ) dφ = 0.

Thus, the integral becomes simply

  I = π J₀(1).

Step 4. Numerical approximation

Using the known value J₀(1) ≈ 0.7651976865579666 and π ≈ 3.141592653589793,
  I ≈ 3.141592653589793 × 0.7651976865579666 ≈ 2.4052847346.

Final answer in JSON format:

{"answer": "\pi J_0(1)", "numerical_answer": "2.4052847346"}