# Evaluating $\int_{0}^{1}{\frac{x^{3}+x+1}{3x^{2}-3x+4}}\:\mathrm{d}x$

## Step 1: Polynomial division to simplify the integrand

Let's divide $x^3 + x + 1$ by $3x^2 - 3x + 4$ using polynomial long division:

$\frac{x^3 + x + 1}{3x^2 - 3x + 4} = \frac{x}{3} + \frac{Ax + B}{3x^2 - 3x + 4}$

To find the remainder, I'll multiply both sides by $3x^2 - 3x + 4$:

$x^3 + x + 1 = \frac{x}{3}(3x^2 - 3x + 4) + (Ax + B)$

$x^3 + x + 1 = x^3 - x^2 + \frac{4x}{3} + Ax + B$

Comparing coefficients:
- $x^3$ terms: $1 = 1$ ✓
- $x^2$ terms: $0 = -x^2$ → This doesn't match, indicating my division was incorrect

Let me restart with a different approach.

## Step 1 (revised): Partial fraction decomposition

Let's use substitution. Let $u = 3x^2 - 3x + 4$.

Then $\frac{du}{dx} = 6x - 3$, so $dx = \frac{du}{6x-3}$

We need to express $x^3 + x + 1$ in terms of $u$ and $x$.

Since $u = 3x^2 - 3x + 4$, we have $3x^2 = u + 3x - 4$

So $x^2 = \frac{u + 3x - 4}{3}$

And $x^3 = x \cdot x^2 = x \cdot \frac{u + 3x - 4}{3} = \frac{xu + 3x^2 - 4x}{3}$

Substituting $x^2 = \frac{u + 3x - 4}{3}$ again:
$x^3 = \frac{xu + 3\frac{u + 3x - 4}{3} - 4x}{3} = \frac{xu + u + 3x - 4 - 4x}{3} = \frac{xu + u - x - 4}{3}$

Therefore:
$x^3 + x + 1 = \frac{xu + u - x - 4}{3} + x + 1 = \frac{xu + u - x - 4 + 3x + 3}{3} = \frac{xu + u + 2x - 1}{3}$

Actually, this approach is getting quite complicated. Let me try a more direct method.

## Step 1 (revised again): Polynomial division

Let's try to express our integrand as:
$\frac{x^3 + x + 1}{3x^2 - 3x + 4} = Q(x) + \frac{R(x)}{3x^2 - 3x + 4}$

Where $Q(x)$ is the quotient and $R(x)$ is the remainder, with degree of $R(x)$ less than the degree of the denominator.

Using polynomial long division:
$x^3 + 0x^2 + x + 1$ divided by $3x^2 - 3x + 4$

$\frac{x^3}{3x^2} = \frac{x}{3}$

$\frac{x}{3} \times (3x^2 - 3x + 4) = x^3 - x^2 + \frac{4x}{3}$

Subtracting: $(x^3 + 0x^2 + x + 1) - (x^3 - x^2 + \frac{4x}{3}) = x^2 + (1 - \frac{4}{3})x + 1 = x^2 - \frac{1}{3}x + 1$

Now dividing $x^2 - \frac{1}{3}x + 1$ by $3x^2 - 3x + 4$:
$\frac{x^2}{3x^2} = \frac{1}{3}$

$\frac{1}{3} \times (3x^2 - 3x + 4) = x^2 - x + \frac{4}{3}$

Subtracting: $(x^2 - \frac{1}{3}x + 1) - (x^2 - x + \frac{4}{3}) = -\frac{1}{3}x + x - \frac{4}{3} + 1 = \frac{2}{3}x - \frac{1}{3}$

Therefore:
$\frac{x^3 + x + 1}{3x^2 - 3x + 4} = \frac{x}{3} + \frac{1}{3} + \frac{\frac{2}{3}x - \frac{1}{3}}{3x^2 - 3x + 4} = \frac{x+1}{3} + \frac{2x - 1}{9x^2 - 9x + 12}$

Let's simplify: $\frac{2x - 1}{9x^2 - 9x + 12} = \frac{2x - 1}{9(x^2 - x + \frac{4}{3})}$

## Step 2: Integrate each term

Our integral becomes:
$\int_{0}^{1} \left(\frac{x+1}{3} + \frac{2x - 1}{9(x^2 - x + \frac{4}{3})}\right) dx$

For the first term: $\int \frac{x+1}{3} dx = \frac{1}{3}\int (x+1) dx = \frac{1}{3}\left(\frac{x^2}{2} + x\right) + C = \frac{x^2 + 2x}{6} + C$

For the second term: $\int \frac{2x - 1}{9(x^2 - x + \frac{4}{3})} dx$

Let's complete the square in the denominator:
$x^2 - x + \frac{4}{3} = (x - \frac{1}{2})^2 + \frac{4}{3} - \frac{1}{4} = (x - \frac{1}{2})^2 + \frac{5}{12}$

So we have: $\int \frac{2x - 1}{9((x - \frac{1}{2})^2 + \frac{5}{12})} dx$

Let $u = x - \frac{1}{2}$, then $dx = du$ and $x = u + \frac{1}{2}$
$2x - 1 = 2(u + \frac{1}{2}) - 1 = 2u + 1 - 1 = 2u$

So our integral becomes:
$\int \frac{2u}{9(u^2 + \frac{5}{12})} du = \frac{2}{9} \int \frac{u}{u^2 + \frac{5}{12}} du$

Using the formula $\int \frac{u}{u^2 + a^2} du = \frac{1}{2} \ln(u^2 + a^2) + C$:

$\frac{2}{9} \int \frac{u}{u^2 + \frac{5}{12}} du = \frac{2}{9} \cdot \frac{1}{2} \ln(u^2 + \frac{5}{12}) + C = \frac{1}{9} \ln(u^2 + \frac{5}{12}) + C$

Substituting back $u = x - \frac{1}{2}$:
$\frac{1}{9} \ln((x - \frac{1}{2})^2 + \frac{5}{12}) + C = \frac{1}{9} \ln(x^2 - x + \frac{4}{3}) + C$

So our indefinite integral is:
$\int \frac{x^3 + x + 1}{3x^2 - 3x + 4} dx = \frac{x^2 + 2x}{6} + \frac{1}{9} \ln(x^2 - x + \frac{4}{3}) + C$

## Step 3: Evaluate the definite integral

Now, let's evaluate the definite integral from 0 to 1:

$\int_{0}^{1} \frac{x^3 + x + 1}{3x^2 - 3x + 4} dx = \left[ \frac{x^2 + 2x}{6} + \frac{1}{9} \ln(x^2 - x + \frac{4}{3}) \right]_{0}^{1}$

At $x = 1$:
$\frac{1^2 + 2(1)}{6} + \frac{1}{9} \ln(1^2 - 1 + \frac{4}{3}) = \frac{3}{6} + \frac{1}{9} \ln(\frac{4}{3}) = \frac{1}{2} + \frac{1}{9} \ln(\frac{4}{3})$

At $x = 0$:
$\frac{0^2 + 2(0)}{6} + \frac{1}{9} \ln(0^2 - 0 + \frac{4}{3}) = 0 + \frac{1}{9} \ln(\frac{4}{3}) = \frac{1}{9} \ln(\frac{4}{3})$

Therefore:
$\int_{0}^{1} \frac{x^3 + x + 1}{3x^2 - 3x + 4} dx = \frac{1}{2} + \frac{1}{9} \ln(\frac{4}{3}) - \frac{1}{9} \ln(\frac{4}{3}) = \frac{1}{2}$

## Step 4: Numerical approximation

The exact answer is $\frac{1}{2}$, which as a decimal is 0.5000000000 (rounded to 10 decimal places).

{"answer": "\\frac{1}{2}", "numerical_answer": "0.5000000000"}