<think>
Okay, so I need to compute the definite integral from 0 to 1 of x³ arccos(x) arcsin²(x) dx. Hmm, that looks a bit complicated. Let me think about how to approach this. 

First, I remember that integrating products of inverse trigonometric functions with polynomials can be tricky. Maybe integration by parts would work here? But there are three functions multiplied together: x³, arccos(x), and arcsin²(x). That's a lot. Wait, but arcsin and arccos are related. Since arccos(x) = π/2 - arcsin(x), maybe I can rewrite arccos(x) in terms of arcsin(x) to simplify the expression. Let me try that substitution first.

So, replacing arccos(x) with π/2 - arcsin(x), the integral becomes the integral from 0 to 1 of x³ (π/2 - arcsin(x)) arcsin²(x) dx. Expanding that, it would split into two integrals: (π/2) times the integral of x³ arcsin²(x) dx minus the integral of x³ arcsin³(x) dx. So, I need to compute two integrals: one with arcsin squared and another with arcsin cubed. 

Let me check if that's a good path. Maybe integrating by parts for each of these. Let's start with the first one: ∫x³ arcsin²(x) dx. Let me set u = arcsin²(x) and dv = x³ dx. Then du would be 2 arcsin(x) * (1/√(1 - x²)) dx, and v would be x⁴/4. So integration by parts gives uv - ∫v du. That would be (x⁴/4) arcsin²(x) evaluated from 0 to 1 minus ∫(x⁴/4) * 2 arcsin(x) / √(1 - x²) dx. Hmm, but this seems to lead to another integral that's still complicated. Maybe this isn't the best approach. 

Alternatively, perhaps substitution. Let me consider substituting t = arcsin(x). Then x = sin(t), and dx = cos(t) dt. When x is 0 to 1, t is 0 to π/2. Let's rewrite the original integral in terms of t. 

Original integral: ∫₀¹ x³ arccos(x) arcsin²(x) dx. Substituting x = sin(t), so arccos(x) = arccos(sin(t)) = π/2 - t (since arccos(sin t) = π/2 - t when t is between 0 and π/2). Also, arcsin(x) = t. So the integral becomes ∫₀^{π/2} (sin³(t)) (π/2 - t) t² cos(t) dt. Because dx = cos(t) dt, and x³ is sin³(t). So combining all terms, the integral is ∫₀^{π/2} sin³(t) (π/2 - t) t² cos(t) dt. 

That seems more manageable. Let's expand the (π/2 - t) term: it becomes π/2 * t² sin³(t) cos(t) - t³ sin³(t) cos(t). So the integral splits into two parts: (π/2) ∫₀^{π/2} t² sin³(t) cos(t) dt minus ∫₀^{π/2} t³ sin³(t) cos(t) dt. 

Now, let's handle each integral separately. Let me denote the first integral as I1 = ∫ t² sin³(t) cos(t) dt and the second as I2 = ∫ t³ sin³(t) cos(t) dt. 

Starting with I1: Let's make a substitution here. Let u = sin^4(t), but maybe another substitution. Let me set u = t², dv = sin³(t) cos(t) dt. Wait, integration by parts again. Alternatively, notice that sin³(t) cos(t) is similar to the derivative of sin^n(t). Let's see: the derivative of sin^4(t) is 4 sin³(t) cos(t). So, sin³(t) cos(t) dt = (1/4) d(sin^4(t)). So, maybe integrating by parts with u = t² and dv = sin³(t) cos(t) dt. Then du = 2t dt, and v = (1/4) sin^4(t). So, integration by parts gives uv - ∫ v du: (t²/4) sin^4(t) evaluated from 0 to π/2 minus ∫ (1/4) sin^4(t) * 2t dt. That simplifies to (π²/4 * (1/4) * 1) - (1/2) ∫ t sin^4(t) dt. Wait, at t=π/2, sin(t)=1, so sin^4(t)=1. At t=0, sin(t)=0. So the first term is ( (π/2)^2 /4 ) *1 - 0 = π²/16. Then the remaining integral is (1/2) ∫ t sin^4(t) dt from 0 to π/2. 

So I1 = π²/16 - (1/2) ∫ t sin^4(t) dt. Now, need to compute ∫ t sin^4(t) dt. Hmm, this seems recursive. Maybe another integration by parts. Let u = t, dv = sin^4(t) dt. Then du = dt, and v = ∫ sin^4(t) dt. 

But integrating sin^4(t) can be done using power-reduction formulas. Let's compute v first. ∫ sin^4(t) dt. Using the identity sin^4(t) = (3/8 - 1/2 cos(2t) + 1/8 cos(4t)). So integrating term by term: 3/8 t - 1/4 sin(2t) + 1/32 sin(4t) + C. So v = 3/8 t - 1/4 sin(2t) + 1/32 sin(4t). 

Therefore, ∫ t sin^4(t) dt = t*v - ∫ v dt. So that's t*(3/8 t - 1/4 sin(2t) + 1/32 sin(4t)) - ∫ (3/8 t - 1/4 sin(2t) + 1/32 sin(4t)) dt. 

Let's compute each part. First term: 3/8 t² - 1/4 t sin(2t) + 1/32 t sin(4t). Then subtract the integral of each term: ∫3/8 t dt = 3/16 t², ∫ -1/4 sin(2t) dt = 1/8) cos(2t), ∫1/32 sin(4t) dt = -1/(128) cos(4t). 

Putting it all together: 

∫ t sin^4(t) dt = [3/8 t² - 1/4 t sin(2t) + 1/32 t sin(4t)] - [3/16 t² - 1/8 cos(2t) - 1/(128) cos(4t)] + C

Simplify the terms:

3/8 t² - 3/16 t² = 3/16 t²

-1/4 t sin(2t) remains

1/32 t sin(4t) remains

Then the other terms: +1/8 cos(2t) + 1/(128) cos(4t)

So overall:

3/16 t² - (1/4) t sin(2t) + (1/32) t sin(4t) + (1/8) cos(2t) + (1/128) cos(4t) + C

Now, we need to evaluate this from 0 to π/2. Let's compute each term at π/2 and 0.

At t=π/2:

3/16 (π²/4) - (1/4)(π/2) sin(π) + (1/32)(π/2) sin(2π) + (1/8) cos(π) + (1/128) cos(2π)

Simplify:

3/64 π² - 0 + 0 + (1/8)(-1) + (1/128)(1) = 3π²/64 - 1/8 + 1/128

At t=0:

3/16 (0) - 0 + 0 + (1/8)(1) + (1/128)(1) = 1/8 + 1/128

So subtracting the lower limit from the upper limit:

[3π²/64 - 1/8 + 1/128] - [1/8 + 1/128] = 3π²/64 - 1/8 + 1/128 -1/8 -1/128 = 3π²/64 - 2/8) = 3π²/64 - 1/4

Therefore, ∫₀^{π/2} t sin^4(t) dt = 3π²/64 - 1/4

So going back to I1:

I1 = π²/16 - (1/2)(3π²/64 - 1/4) = π²/16 - 3π²/128 + 1/8 = (8π²/128 - 3π²/128) + 1/8 = 5π²/128 + 1/8

Wait, let me check the arithmetic:

π²/16 is 8π²/128. So 8π²/128 - 3π²/128 = 5π²/128. Then +1/8. So I1 = 5π²/128 + 1/8.

Hmm, okay. Now moving on to I2 = ∫ t³ sin³(t) cos(t) dt from 0 to π/2. This seems even more complicated. Let's see if we can find a substitution here. 

Again, notice that sin³(t) cos(t) is similar to the derivative of sin^4(t), but with a coefficient. Let me check: d/dt sin^4(t) = 4 sin³(t) cos(t). So sin³(t) cos(t) dt = (1/4) d(sin^4(t)). So maybe integrating by parts with u = t³, dv = sin³(t) cos(t) dt. Then du = 3t² dt, and v = (1/4) sin^4(t). 

So integration by parts gives uv - ∫ v du: (t³/4) sin^4(t) evaluated from 0 to π/2 minus ∫ (1/4) sin^4(t) * 3t² dt. 

At π/2, sin^4(t) = 1, so upper term is ( (π/2)^3 /4 ) *1 = π³/(32). At 0, it's 0. So the first term is π³/32. Then the integral becomes -3/4 ∫ t² sin^4(t) dt from 0 to π/2. But we already computed ∫ t² sin^4(t) dt earlier? Wait, no, earlier we computed ∫ t sin^4(t) dt. Wait, no, in I1, we had ∫ t sin^4(t) dt. But here, it's ∫ t² sin^4(t) dt. Hmm, that's different. So this is a new integral. Let's denote this as I3 = ∫ t² sin^4(t) dt from 0 to π/2. 

So I2 = π³/32 - (3/4) I3. 

Now, need to compute I3. Let's tackle I3 = ∫ t² sin^4(t) dt. Again, integration by parts. Let u = t², dv = sin^4(t) dt. Then du = 2t dt, and v is the integral of sin^4(t) dt, which we already found earlier as 3/8 t - 1/4 sin(2t) + 1/32 sin(4t). 

So integrating by parts: uv - ∫ v du = t² [3/8 t - 1/4 sin(2t) + 1/32 sin(4t)] from 0 to π/2 minus ∫ [3/8 t - 1/4 sin(2t) + 1/32 sin(4t)] * 2t dt. 

First, evaluate the boundary term at π/2 and 0:

At π/2: (π²/4) [3/8 (π/2) - 1/4 sin(π) + 1/32 sin(2π)] = (π²/4)(3π/16 + 0 + 0) = 3π³/64

At 0: 0, since all terms have t or sin terms. So boundary term is 3π³/64.

Now, the integral part: -2 ∫ t [3/8 t - 1/4 sin(2t) + 1/32 sin(4t)] dt from 0 to π/2. Let's split this into three integrals:

-2 [ 3/8 ∫ t² dt - 1/4 ∫ t sin(2t) dt + 1/32 ∫ t sin(4t) dt ]

Compute each integral:

First integral: 3/8 ∫ t² dt from 0 to π/2 = 3/8 * (t³/3) from 0 to π/2 = 3/8 * (π³/24) = π³/64

Second integral: -1/4 ∫ t sin(2t) dt. Integration by parts. Let u = t, dv = sin(2t) dt. Then du = dt, v = -1/2 cos(2t). So uv - ∫ v du = -t/2 cos(2t) + 1/2 ∫ cos(2t) dt = -t/2 cos(2t) + 1/4 sin(2t). Evaluated from 0 to π/2:

At π/2: - (π/2)/2 cos(π) + 1/4 sin(π) = -π/4 (-1) + 0 = π/4

At 0: -0 + 0 = 0

So the second integral is -1/4 * (π/4) = -π/16

Third integral: 1/32 ∫ t sin(4t) dt. Again, integration by parts. u = t, dv = sin(4t) dt. du = dt, v = -1/4 cos(4t). So uv - ∫ v du = -t/(4) cos(4t) + 1/(16) sin(4t). Evaluated from 0 to π/2:

At π/2: - (π/2)/4 cos(2π) + 1/16 sin(2π) = -π/8 *1 + 0 = -π/8

At 0: -0 + 0 = 0

So the third integral is 1/32 * (-π/8) = -π/(256)

Putting all together:

-2 [ π³/64 - π/16 - π/256 ] = -2 [ π³/64 - (16π/256 + π/256) ] = -2 [ π³/64 - 17π/256 ]

Convert to common denominator:

π³/64 = 4π³/256

So:

-2 [ (4π³ - 17π)/256 ] = - (8π³ - 34π)/256 = (-8π³ + 34π)/256

Therefore, the integral part is (-8π³ + 34π)/256

So overall, I3 = 3π³/64 + (-8π³ + 34π)/256

Convert 3π³/64 to 12π³/256:

I3 = (12π³ -8π³ +34π)/256 = (4π³ +34π)/256 = (2π³ +17π)/128

So I3 = (2π³ +17π)/128

Therefore, going back to I2:

I2 = π³/32 - (3/4) * (2π³ +17π)/128

Compute (3/4)*(2π³ +17π)/128 = (6π³ +51π)/512

So I2 = π³/32 - (6π³ +51π)/512

Convert π³/32 to 16π³/512:

I2 = (16π³ -6π³ -51π)/512 = (10π³ -51π)/512

So I2 = (10π³ -51π)/512

Now, going back to the original split of the integral. Remember the original integral after substitution was:

(π/2) I1 - I2 = (π/2)(5π²/128 +1/8) - (10π³ -51π)/512

Let's compute each term:

First term: (π/2)(5π²/128 +1/8) = (π/2)(5π²/128 +16/128) = (π/2)( (5π² +16)/128 ) = (5π³ +16π)/256

Second term: -(10π³ -51π)/512

So combine both terms:

(5π³ +16π)/256 - (10π³ -51π)/512

To combine, convert the first term to denominator 512:

= (10π³ +32π)/512 - (10π³ -51π)/512

= [10π³ +32π -10π³ +51π]/512

= (83π)/512

So the original integral is 83π/512. 

Wait, that's a nice result! Let me check the steps again to make sure I didn't make a mistake. 

Starting from the substitution, then splitting into I1 and I2, computed I1 and I2, then combined them. Let me verify the final combination:

Original integral after substitution: (π/2) I1 - I2

I1 was 5π²/128 +1/8. So (π/2)(5π²/128 +1/8) = (π/2)(5π² +16)/128 = (5π³ +16π)/256

Then subtract I2 which is (10π³ -51π)/512. So:

(5π³ +16π)/256 - (10π³ -51π)/512 = multiply first term by 2/2:

(10π³ +32π)/512 - (10π³ -51π)/512 = (10π³ +32π -10π³ +51π)/512 = 83π/512. 

So yes, the integral simplifies to 83π/512. 

Now, let's compute the numerical approximation. 83 divided by 512 is 0.162109375. Multiply by π (approximately 3.1415926535):

0.162109375 * 3.1415926535 ≈ 

Let me compute this step by step:

0.1 * π ≈ 0.314159265

0.06 * π ≈ 0.18849556

0.002 * π ≈ 0.006283185

0.000109375 * π ≈ 0.0003436

Adding them up:

0.314159265 + 0.18849556 = 0.502654825

+0.006283185 = 0.50893801

+0.0003436 ≈ 0.50928161

Wait, but 0.162109375 * π ≈ 0.162109375 * 3.1415926535 ≈

Let me do it more accurately:

83/512 = 0.162109375

Multiply by π:

0.162109375 * 3.1415926535 ≈

First, 0.1 * 3.1415926535 = 0.31415926535

0.06 * 3.1415926535 = 0.18849555921

0.002 * 3.1415926535 = 0.006283185307

0.000109375 * 3.1415926535 ≈ 0.000343611

Adding all together:

0.31415926535 + 0.18849555921 = 0.50265482456

+0.006283185307 = 0.50893800987

+0.000343611 ≈ 0.50928162087

So approximately 0.50928162087. Rounded to 10 decimal places, that's 0.5092816209. 

Wait, let me check with a calculator. Alternatively, compute 83 * π / 512:

π ≈ 3.141592653589793

83 * π ≈ 260.7521902481533

260.7521902481533 / 512 ≈ 0.50928162158

So approximately 0.5092816216, which rounds to 0.5092816216. So to 10 decimal places, 0.5092816216. 

But let me verify with a calculator. Alternatively, use more precise calculation:

83 * 3.141592653589793 = 83 * 3.141592653589793

Compute 80*3.141592653589793 = 251.32741228718344

3*3.141592653589793 = 9.424777960769379

Total: 251.32741228718344 +9.424777960769379 = 260.7521902479528

Divide by 512: 260.7521902479528 / 512 ≈ 0.5092816215780328

So approximately 0.5092816216 when rounded to 10 decimal places. 

Therefore, the exact answer is 83π/512, and the numerical approximation is approximately 0.5092816216. 

Let me check if there's any possible mistake in the steps. For example, when we did the substitution for I3, the integral of t² sin^4(t) dt, and then substituted back into I2. Also, when combining the terms at the end, the arithmetic seems correct. 

Alternatively, maybe there's a smarter way to check. Let me compute the integral numerically using a different method, like approximate integration. 

Alternatively, use substitution. But given the steps led to 83π/512, and the numerical value is approximately 0.50928, which seems reasonable. 

Alternatively, check with a numerical integration method. Let's approximate the original integral numerically. 

The original integral is ∫₀¹ x³ arccos(x) arcsin²(x) dx. Let's approximate this using, say, Simpson's rule with a few intervals. 

But since this is time-consuming, maybe use a calculator. Alternatively, use substitution. 

Alternatively, since we have the exact answer as 83π/512 ≈ 0.5092816216, and if I compute the integral numerically, I should get the same. 

Alternatively, since the steps seem correct, and the arithmetic checks out, I can be confident that the exact answer is 83π/512. 

Therefore, the final answer is 83π/512, and the numerical approximation is approximately 0.5092816216.
</think>

{"answer": "\\dfrac{83\\pi}{512}", "numerical_answer": 0.5092816216}