To solve the definite integral \(\int\limits_0^2 x H_{3}\left(\sqrt{x(2-x)}\right) dx\), we follow these steps:

### Step 1: Understand the Hermite Polynomial \(H_3(y)\)
The Hermite polynomial \(H_3(y)\) is given by:
\[
H_3(y) = 8y^3 - 12y
\]
Thus, the integrand becomes:
\[
x H_3\left(\sqrt{x(2-x)}\right) = x \left[8\left(\sqrt{x(2-x)}\right)^3 - 12\sqrt{x(2-x)}\right] = 8x \left(x(2-x)\right)^{3/2} - 12x \sqrt{x(2-x)}
\]

### Step 2: Simplify the Integrand
Letâ€™s rewrite the integrand:
\[
8x \left(x(2-x)\right)^{3/2} - 12x \sqrt{x(2-x)} = 8x^{5/2} (2-x)^{3/2} - 12x^{3/2} (2-x)^{1/2}
\]

### Step 3: Substitute to Simplify the Integral
Let \(x = 2\sin^2\theta\), then \(dx = 4\sin\theta\cos\theta d\theta\), and the limits change from \(x=0\) to \(\theta=0\) and \(x=2\) to \(\theta=\pi/2\).

Substituting:
\[
x^{5/2} = (2\sin^2\theta)^{5/2} = 2^{5/2} \sin^5\theta
\]
\[
(2-x)^{3/2} = (2 - 2\sin^2\theta)^{3/2} = (2\cos^2\theta)^{3/2} = 2^{3/2} \cos^3\theta
\]
\[
x^{3/2} = (2\sin^2\theta)^{3/2} = 2^{3/2} \sin^3\theta
\]
\[
(2-x)^{1/2} = (2\cos^2\theta)^{1/2} = \sqrt{2} \cos\theta
\]

Thus, the integrand becomes:
\[
8 \cdot 2^{5/2} \sin^5\theta \cdot 2^{3/2} \cos^3\theta \cdot 4\sin\theta\cos\theta - 12 \cdot 2^{3/2} \sin^3\theta \cdot \sqrt{2} \cos\theta \cdot 4\sin\theta\cos\theta
\]
Simplifying:
\[
8 \cdot 2^{4} \sin^6\theta \cos^4\theta - 12 \cdot 2^{2} \sin^4\theta \cos^2\theta
\]

### Step 4: Evaluate the Integral
The integral becomes:
\[
\int_0^{\pi/2} \left[128 \sin^6\theta \cos^4\theta - 48 \sin^4\theta \cos^2\theta\right] d\theta
\]
Using the identity for integrals of powers of sine and cosine:
\[
\int_0^{\pi/2} \sin^m\theta \cos^n\theta d\theta = \frac{\Gamma\left(\frac{m+1}{2}\right) \Gamma\left(\frac{n+1}{2}\right)}{2 \Gamma\left(\frac{m+n+2}{2}\right)}
\]
We compute:
\[
128 \cdot \frac{\Gamma(7/2) \Gamma(5/2)}{2 \Gamma(6)} - 48 \cdot \frac{\Gamma(5/2) \Gamma(3/2)}{2 \Gamma(4)}
\]
Simplifying with \(\Gamma(n+1) = n\Gamma(n)\) and \(\Gamma(1/2) = \sqrt{\pi}\):
\[
128 \cdot \frac{\frac{15}{8}\sqrt{\pi} \cdot \frac{3}{4}\sqrt{\pi}}{2 \cdot 120} - 48 \cdot \frac{\frac{3}{4}\sqrt{\pi} \cdot \frac{1}{2}\sqrt{\pi}}{2 \cdot 6} = \frac{3\pi}{2}
\]

### Step 5: Numerical Approximation
The exact answer is \(\frac{3\pi}{2}\), which numerically approximates to:
\[
4.7123889804
\]

### Final Answer
```json
{"answer": "\\frac{3\\pi}{2}", "numerical_answer": "4.7123889804"}
```