<think>
Okay, let's see. I need to compute the definite integral of x squared times the cube root of (x cubed plus 1) from -1 to 1. Hmm, the function is x²·∛(x³+1). Alright, first step is to think about substitution. The cube root is the same as raising to the 1/3 power, so maybe that's a hint. Let me try substitution.

Let u be the inside of the cube root, so u = x³ + 1. Then du/dx = 3x². Oh, wait, the integrand has x² dx. So if I set u = x³ + 1, then du = 3x² dx, which means x² dx is du/3. That seems promising. Let's check the limits. When x is -1, u = (-1)^3 + 1 = -1 + 1 = 0. When x is 1, u = 1^3 + 1 = 2. So the integral becomes from u=0 to u=2 of ∛u * (du/3). So that's (1/3) ∫ from 0 to 2 of u^(1/3) du. 

Integrating u^(1/3) is straightforward. The integral of u^(n) is u^(n+1)/(n+1), so here n=1/3. So that becomes (1/3) * [u^(4/3)/(4/3)] from 0 to 2. Simplify that: (1/3) * (3/4) [u^(4/3)] from 0 to 2. The 1/3 and 3/4 cancel out to 1/4. So it's (1/4)(2^(4/3) - 0^(4/3)). Since 0^(4/3) is 0, the integral is (1/4)*2^(4/3). 

Now, 2^(4/3) can be written as 2^(1 + 1/3) = 2*2^(1/3). So 2^(4/3) = 2 * cube root of 2. Therefore, the exact answer is (1/4)*2*2^(1/3) = (1/2)*2^(1/3). Alternatively, 2^(1/3)/2. But maybe it's better to write it as (2^(4/3))/4. Either way, that's the exact value.

For the numerical approximation, let's compute 2^(1/3). The cube root of 2 is approximately 1.259921049894873. Multiply that by 2: 2.519842099789746. Then divide by 4: 0.6299605249. Wait, but let me check again. Wait, 2^(4/3) is 2^(1 + 1/3) = 2 * 2^(1/3). So 2^(1/3) ≈1.25992105, so 2*1.25992105 ≈2.5198421. Then divide by 4: 2.5198421 /4 ≈0.629960525. So rounding to 10 decimal places, that's 0.6299605249... Let me check with a calculator. Alternatively, compute 2^(4/3) first. 2^(4/3) = e^( (4/3) ln 2 ). ln 2 ≈0.6931471806. Multiply by 4/3: 0.6931471806 * 4/3 ≈0.9241962408. Then e^0.9241962408 ≈2.519842099. Then divide by 4: 2.519842099 /4 ≈0.6299605247. So approximately 0.6299605247. Rounded to 10 decimal places, that's 0.6299605247. Let me confirm with another method. Alternatively, use a calculator for 2^(4/3)/4. Let me compute 2^(1/3) first. 2^(1/3) is approximately 1.2599210498948732. Then 2^(4/3) is (2^(1/3))^4? Wait, no. Wait, 2^(4/3) is 2^(1 + 1/3) = 2 * 2^(1/3). So 2*1.2599210498948732 ≈2.5198420997897464. Then divide by 4: 2.5198420997897464 /4 ≈0.6299605249474366. So rounding to 10 decimal places, that's 0.6299605249. Wait, but the exact digits after decimal: 0.6299605249 (first 10 digits: 0.6299605249...). So the numerical approximation is approximately 0.6299605249.

Wait, let me check if I did the substitution correctly. The original integral is from -1 to 1. But when x is negative, like x=-1, u becomes 0, and when x=1, u=2. But the substitution seems valid here. The function x² is even, but the cube root of (x³ +1) is not even. However, the substitution worked because the x² dx part is part of du. So the substitution should be correct. Let me check with x=-0.5. If x=-0.5, then x^3 is -0.125, so u=0.875. But when x is negative, does the substitution still hold? Let's see. The substitution u = x³ +1 is valid for all x, and the integral from -1 to 1 becomes u from 0 to 2. So the substitution is correct. Therefore, the integral is indeed (1/4) * 2^(4/3). So exact answer is 2^(4/3)/4. Which can be written as \frac{2^{4/3}}{4} or simplified to \frac{2^{1/3}}{2} but maybe the first form is better. Alternatively, 2^(4/3) is 2^(1 +1/3) = 2*2^(1/3), so 2*2^(1/3)/4 = 2^(1/3)/2. So both forms are correct. Let me check which is simpler. 2^(4/3)/4 is the same as 2^(4/3 - 2) = 2^(-2/3), but wait, 4 is 2^2, so 2^(4/3)/2^2 = 2^(4/3 - 2) = 2^(-2/3) = 1/(2^(2/3)). Wait, that's another way. Wait, 2^(4/3)/4 = 2^(4/3)/2^2 = 2^(4/3 - 2) = 2^(-2/3) = 1/(2^(2/3)). But 2^(2/3) is cube root of 4. So 1 over cube root of 4. But that's equivalent to 2^(1/3)/2. Let me verify: 2^(1/3)/2 = 2^(1/3 -1) = 2^(-2/3) = 1/(2^(2/3)). So both forms are equivalent. So perhaps writing it as \frac{\sqrt[3]{2}}{2} is simpler. But maybe the original form is better. Let me see. The integral is (1/4)*2^(4/3). So 2^(4/3)/4. Alternatively, 2^(4/3) is 2*2^(1/3), so 2*2^(1/3)/4 = 2^(1/3)/2. So both forms are correct. So which one to choose? Maybe the problem expects the answer in the form with exponents, so 2^(4/3)/4. Alternatively, simplifying exponents: 2^(4/3 - 2) = 2^(-2/3) = 1/(2^(2/3)). But that's the same as 1 over cube root of 4. Hmm. But perhaps the first form is better. Let me check. Let's compute 2^(4/3)/4. So 2^(4/3) is 2^(1 +1/3) = 2 * 2^(1/3). So 2*2^(1/3)/4 = (2/4)*2^(1/3) = (1/2)*2^(1/3). So that's the same as 2^(1/3)/2. So both forms are equivalent. So maybe the answer as \frac{2^{4/3}}{4} or \frac{\sqrt[3]{2}}{2}. Either is acceptable, but perhaps the first is more direct from the integral calculation. Let me confirm. The integral was (1/4) * 2^(4/3). So writing that as \frac{2^{4/3}}{4} is correct. Alternatively, simplifying exponents: 2^(4/3) divided by 4 is 2^(4/3 - 2) = 2^(-2/3) = 1/(2^(2/3)) = 1/\sqrt[3]{4}. But that's another form. So which is better? The problem says to put the exact answer in LaTeX. So perhaps the simplest form is \frac{2^{4/3}}{4} or \frac{\sqrt[3]{16}}{4} since 2^4 is 16, so 16^(1/3)/4. Wait, 16^(1/3) is 2^(4/3). Hmm. Alternatively, maybe the problem expects the answer in terms of cube roots. Let me see. 2^(4/3) is 2^(1 +1/3) = 2 * 2^(1/3). So 2*2^(1/3)/4 = (2/4)*2^(1/3) = (1/2)*2^(1/3). So that's the same as 2^(1/3)/2. So maybe writing it as \frac{\sqrt[3]{2}}{2} is simpler. Let me check if that's correct. Let's compute 2^(1/3)/2. 2^(1/3) is cube root of 2, so cube root of 2 divided by 2. Yes. So both forms are correct. Which one is preferable? The problem might prefer the answer in terms of exponents, but both are acceptable. Let me check with the substitution steps. The integral became (1/4) * u^(4/3) evaluated from 0 to 2. So (1/4)(2^(4/3) - 0) = 2^(4/3 /4). So the exact answer is 2^(4/3)/4. So I think that's the most direct form. So I'll go with \boxed{\dfrac{2^{4/3}}{4}} for the exact answer, and the numerical approximation is approximately 0.6299605249.

Wait, but let me check if the substitution is valid for x from -1 to 1. The function x² is always non-negative, and the cube root function is defined for all real numbers. So when x is negative, x³ +1 can be negative or positive. For example, when x is between -1 and 0, x³ is between -1 and 0, so x³ +1 is between 0 and 1. When x is between 0 and 1, x³ +1 is between 1 and 2. So the cube root is defined for all these values. So the substitution is valid. Also, the substitution u = x³ +1 is differentiable and bijective over the interval? Well, the derivative is 3x², which is non-negative except at x=0. But since x² is non-negative, the substitution is increasing from x=-1 to x=1. Wait, when x increases from -1 to 1, u increases from 0 to 2. So the substitution is valid. Therefore, the integral is correctly transformed. So the exact answer is 2^(4/3)/4, and the numerical value is approximately 0.6299605249.
</think>

{"answer": "\\dfrac{2^{4/3}}{4}", "numerical_answer": 0.6299605249}