We wish to evaluate

  I = ∫₀¹ [ln(x + 1/x)]/(x + 1/x) dx.

A useful first step is to rewrite the logarithm. Observe that

  ln(x + 1/x) = ln[(x² + 1)/x] = ln(1 + x²) – ln x.

Also, notice that
  x + 1/x = (x² + 1)/x.
Thus the integrand becomes

  [ln(1 + x²) – ln x] / ((x² + 1)/x)
    = x · [ln(1 + x²) – ln x] / (1 + x²).

That is, we may split I into two integrals:
  I = I₁ – I₂,
with
  I₁ = ∫₀¹ [x ln(1 + x²)]/(1 + x²) dx  and  I₂ = ∫₀¹ [x ln x]/(1 + x²) dx.

Step 1. Evaluation of I₁

Make the substitution u = x² so that du = 2x dx, or x dx = du/2. When x goes from 0 to 1, u goes from 0 to 1. Then
  I₁ = ∫₀¹ [x ln(1+x²)]/(1+x²) dx
    = ½ ∫₀¹ [ln(1 + u)]/(1 + u) du.
Now set v = 1 + u ⇒ dv = du and when u = 0, v = 1; when u = 1, v = 2. Thus,
  I₁ = ½ ∫₁² (ln v)/v dv.
But we know that
  ∫ (ln v)/v dv = ½ (ln v)² + C.
So,
  I₁ = ½ · [½ (ln v)²]₍ᵥ₌₁₎² = ¼ [(ln 2)² – (ln 1)²] = (ln 2)²/4,
since ln 1 = 0.

Step 2. Evaluation of I₂

We now need to evaluate
  I₂ = ∫₀¹ [x ln x]/(1+x²) dx.
A convenient method is to introduce a parameter. Define
  J(a) = ∫₀¹ xᵃ/(1+x²) dx.
Then, differentiating with respect to a gives
  J′(a) = ∫₀¹ xᵃ ln x/(1+x²) dx.
Thus, I₂ = J′(1).

To compute J(a) we write
  J(a) = ∫₀¹ xᵃ/(1+x²) dx = ∑ₙ₌₀^∞ (-1)ⁿ ∫₀¹ x^(a+2n) dx   (expanding 1/(1+x²) as a geometric series valid for x ∈ [0,1]).
Since
  ∫₀¹ x^(a+2n) dx = 1/(a+2n+1),
it follows that
  J(a) = ∑ₙ₌₀^∞ (-1)ⁿ/(a+2n+1).

Differentiate term‐by‐term:
  J′(a) = –∑ₙ₌₀^∞ (-1)ⁿ/(a+2n+1)².
In particular, at a = 1 we have
  I₂ = J′(1) = –∑ₙ₌₀^∞ (-1)ⁿ/(2n+2)².
Writing 2n+2 = 2(n+1), we have
  I₂ = –∑ₙ₌₀^∞ (-1)ⁿ/(4 (n+1)²) = –1/4 ∑ₘ₌₁^∞ (-1)^(m–1)/m²,
where we made the substitution m = n + 1.

A standard result is that
  ∑ₘ₌₁^∞ (-1)^(m–1)/m² = π²/12.
Thus,
  I₂ = –1/4 · (π²/12) = –π²/48.

Step 3. Combining the results

We obtained
  I₁ = (ln 2)²/4  and  I₂ = –π²/48.
Thus,
  I = I₁ – I₂ = (ln 2)²/4 – (–π²/48) = (ln 2)²/4 + π²/48.

Step 4. Numerical approximation

Now we compute a numerical approximation. We have
  ln 2 ≈ 0.6931471806, so (ln 2)² ≈ 0.4804530139, and (ln 2)²/4 ≈ 0.1201132535.
Also, π² ≈ 9.8696044011, so π²/48 ≈ 0.2052000917.
Thus, the total is approximately
  I ≈ 0.1201132535 + 0.2052000917 = 0.3253133452.

The final answer in the required format is:

{"answer": "\\frac{\\pi^2}{48}+\\frac{(\\ln 2)^2}{4}", "numerical_answer": "0.3253133452"}