
To solve the definite integral \(\int_0^\pi \sec x \ln\left(1+\frac{\cos x}{3}\right) \, dx\), we proceed as follows:

### Step 1: Expand the Logarithm as a Power Series
The integrand involves \(\ln\left(1+\frac{\cos x}{3}\right)\). For \(|y| < 1\), the Taylor series expansion of \(\ln(1+y)\) is \(\sum_{n=1}^\infty \frac{(-1)^{n+1} y^n}{n}\). Here, \(y = \frac{\cos x}{3}\), and since \(|\cos x| \leq 1\), we have \(|y| \leq \frac{1}{3} < 1\), so the expansion is valid:
\[
\ln\left(1+\frac{\cos x}{3}\right) = \sum_{n=1}^\infty \frac{(-1)^{n+1} (\cos x)^n}{n \cdot 3^n}.
\]

### Step 2: Simplify the Integrand
The integrand becomes:
\[
\sec x \cdot \ln\left(1+\frac{\cos x}{3}\right) = \frac{1}{\cos x} \cdot \sum_{n=1}^\infty \frac{(-1)^{n+1} (\cos x)^n}{n \cdot 3^n} = \sum_{n=1}^\infty \frac{(-1)^{n+1} (\cos x)^{n-1}}{n \cdot 3^n}.
\]

### Step 3: Interchange Sum and Integral
By uniform convergence (justified by the Weierstrass M-test), we interchange the sum and integral:
\[
\int_0^\pi \sec x \ln\left(1+\frac{\cos x}{3}\right) dx = \sum_{n=1}^\infty \frac{(-1)^{n+1}}{n \cdot 3^n} \int_0^\pi (\cos x)^{n-1} dx.
\]

### Step 4: Evaluate the Integral of \((\cos x)^{k}\)
For \(k = n-1\), consider two cases:
- If \(k\) is odd (\(n\) even), \(\int_0^\pi (\cos x)^k dx = 0\) (due to symmetry).
- If \(k\) is even (\(n\) odd), let \(k = 2m\) (so \(n = 2m+1\)). Then:
\[
\int_0^\pi (\cos x)^{2m} dx = \pi \cdot \frac{(2m-1)!!}{(2m)!!} = \pi \cdot \frac{\binom{2m}{m}}{4^m},
\]
where \((2m)!! = 2^m m!\) and \((2m-1)!! = \frac{(2m)!}{2^m m!}\).

### Step 5: Simplify the Series
Only odd \(n\) contribute. Let \(n = 2m+1\) (so \(m \geq 0\)). The series becomes:
\[
\sum_{m=0}^\infty \frac{(-1)^{2m+2}}{(2m+1) \cdot 3^{2m+1}} \cdot \pi \cdot \frac{\binom{2m}{m}}{4^m} = \frac{\pi}{3} \sum_{m=0}^\infty \frac{\binom{2m}{m}}{(2m+1) \cdot 36^m}.
\]

### Step 6: Recognize the Series as an Integral
The sum \(\sum_{m=0}^\infty \frac{\binom{2m}{m} x^m}{2m+1}\) can be evaluated using the generating function for central binomial coefficients. For \(x = \frac{1}{36}\), this sum equals \(3 \arcsin\left(\frac{1}{3}\right)\) (verified by integrating the generating function).

### Step 7: Final Result
Thus, the integral simplifies to:
\[
\frac{\pi}{3} \cdot 3 \arcsin\left(\frac{1}{3}\right) = \pi \arcsin\left(\frac{1}{3}\right).
\]

### Numerical Approximation
Using \(\arcsin\left(\frac{1}{3}\right) \approx 0.3398368369\), the numerical value is:
\[
\pi \cdot 0.3398368369 \approx 1.0676232350.
\]

{"answer": "\(\pi \arcsin\left(\frac{1}{3}\right)\)", "numerical_answer": "1.0676232350"}