<think>
Okay, so I need to compute the definite integral of cos(x + cos x) from 0 to π. Let me start by thinking about how to approach this. Hmm, integrating cos of a function that includes both x and cos x inside... That seems tricky. I remember that integrals involving cos(cos x) or similar expressions often don't have elementary antiderivatives. Let me check if there's a substitution or some identity that could help here.

First, maybe expand the cosine of a sum. Using the cosine addition formula: cos(a + b) = cos a cos b - sin a sin b. So, applying that here, cos(x + cos x) would be cos x cos(cos x) - sin x sin(cos x). So the integral becomes the integral from 0 to π of [cos x cos(cos x) - sin x sin(cos x)] dx. Let me write that into two separate integrals:

∫₀^π cos x cos(cos x) dx - ∫₀^π sin x sin(cos x) dx.

Now, let's look at each part. The first integral is ∫ cos x cos(cos x) dx. Maybe substitution? Let me try u = sin x. Wait, but the argument inside the cosine is cos x. Alternatively, maybe u = cos x. Let's try that for the first integral. Let u = cos x, then du/dx = -sin x. Hmm, but the integral has cos x times cos(cos x) dx. So, if u = cos x, du = -sin x dx. But here, the integrand is cos x * cos(u) dx. Not sure if that helps. Let me see:

Wait, maybe integration by parts? Let's consider the first integral: ∫ cos x cos(cos x) dx. Let me set u = cos(cos x), dv = cos x dx. Then du/dx = sin(cos x) * sin x (by chain rule), and v = sin x. So integration by parts gives uv - ∫ v du. So that would be sin x cos(cos x) - ∫ sin x * sin(cos x) * sin x dx. Wait, but the second term becomes ∫ sin²x sin(cos x) dx. That seems more complicated. Maybe not helpful.

Alternatively, maybe look at the second integral: ∫ sin x sin(cos x) dx. Let me try substitution here. Let u = cos x, then du = -sin x dx. So that integral becomes -∫ sin(cos x) du. But u = cos x, so sin(cos x) is sin u. Wait, so the integral becomes -∫ sin u du = cos u + C = cos(cos x) + C. So the integral of sin x sin(cos x) dx from 0 to π would be -cos(cos x) evaluated from 0 to π. Let me check that.

Wait, substitution: Let u = cos x, then when x=0, u=cos 0=1; when x=π, u=cos π = -1. So the integral becomes ∫ from u=1 to u=-1 of sin u (-du) (because du = -sin x dx, so sin x dx = -du). So that's ∫ from 1 to -1 of sin u (-du) = ∫ from -1 to 1 of sin u du. The integral of sin u is -cos u, so evaluated from -1 to 1: (-cos 1) - (-cos(-1)) = -cos 1 + cos(-1). But cos is even, so cos(-1) = cos 1. Therefore, this becomes -cos 1 + cos 1 = 0. Wait, so the second integral is zero?

Wait, let me verify again. The integral ∫₀^π sin x sin(cos x) dx. Let u = cos x, du = -sin x dx. So the integral becomes ∫_{u=1}^{u=-1} sin u (-du) = ∫_{-1}^1 sin u du. The integral of sin u is -cos u, so from -1 to 1: (-cos 1) - (-cos(-1)) = -cos 1 + cos 1 = 0. Yes, that's correct. So the second integral is zero. So the original integral becomes the first integral minus zero, so just the first integral: ∫₀^π cos x cos(cos x) dx.

Now, how to compute ∫ cos x cos(cos x) dx from 0 to π. Hmm. Let's see. Maybe another substitution? Let me try substitution here. Let’s set t = x - π/2, but not sure. Alternatively, maybe expand cos(cos x) as a series? Since integrating term by term might be possible. Wait, but the problem says to compute the integral analytically. If it's possible, maybe there's a trick.

Alternatively, consider the function f(x) = cos(x + cos x). Let me check if it's an odd or even function around some point. The interval is from 0 to π. Let me see if there's symmetry. Let’s substitute x = π - y. Let’s let y = π - x. When x=0, y=π; when x=π, y=0. Then dx = -dy. The integral becomes ∫ from y=π to y=0 of cos(π - y + cos(π - y)) (-dy) = ∫₀^π cos(π - y + cos(π - y)) dy. Now, cos(π - y) = -cos y, so the argument inside the cosine becomes π - y - cos y. Then cos(π - y - cos y) = cos(π - (y + cos y)) = -cos(y + cos y) because cos(π - θ) = -cos θ. So the integral becomes ∫₀^π -cos(y + cos y) dy. But the original integral is ∫₀^π cos(x + cos x) dx. So we have that I = ∫₀^π cos(x + cos x) dx = ∫₀^π -cos(y + cos y) dy = -I. Therefore, I = -I, which implies that 2I = 0, so I = 0. Wait, is that possible?

Wait, let me check that substitution again. Let me do it step by step. Let’s perform substitution x = π - t. Then when x=0, t=π; when x=π, t=0. Then dx = -dt. The integral becomes:

∫_{x=0}^{π} cos(x + cos x) dx = ∫_{t=π}^{0} cos(π - t + cos(π - t)) (-dt) = ∫_{0}^{π} cos(π - t + cos(π - t)) dt.

Now, cos(π - t) = -cos t, so the argument inside the cosine is π - t + (-cos t) = π - (t + cos t). Then, using the identity cos(π - θ) = -cos θ, we have:

cos(π - (t + cos t)) = -cos(t + cos t).

Therefore, the integral becomes ∫₀^π -cos(t + cos t) dt = -∫₀^π cos(t + cos t) dt = -I.

But the original integral is I, so we have I = -I, which implies 2I = 0, so I = 0. Therefore, the integral is zero. Wait, that's the conclusion? So the integral of cos(x + cos x) from 0 to π is zero? That seems surprising, but maybe due to symmetry.

But let me verify this with a numerical approximation. Let's compute the integral numerically to check. Let's take some sample values. For example, at x=0, cos(0 + cos 0) = cos(0 + 1) = cos(1) ≈ 0.5403. At x=π/2, cos(π/2 + cos(π/2)) = cos(π/2 + 0) = cos(π/2) = 0. At x=π, cos(π + cos π) = cos(π + (-1)) = cos(π -1) ≈ cos(2.1416) ≈ -0.5403. So the function starts at ~0.54, goes to 0 at π/2, then to ~-0.54 at π. The area under the curve from 0 to π might indeed be zero if the positive and negative areas cancel out. But is that the case?

Wait, but the function is symmetric around π/2? Let me check. Let’s take x and π - x. For x in [0, π/2], the corresponding point π - x is in [π/2, π]. Let’s compute cos(x + cos x) and cos(π - x + cos(π - x)). The latter is cos(π - x + (-cos x)) = cos(π - x - cos x). Using the identity cos(π - θ) = -cos θ, but here θ = x + cos x. Wait, but π - x - cos x = π - (x + cos x). So cos(π - (x + cos x)) = -cos(x + cos x). Therefore, the function at π - x is -cos(x + cos x). So the function is odd around x = π/2. Therefore, integrating from 0 to π would result in zero because each x in [0, π/2] pairs with π - x in [π/2, π], and their contributions cancel each other. Therefore, the integral is indeed zero.

So the analytical result is zero, and the numerical approximation would also be zero. Let me check with a simple numerical method. For example, using the trapezoidal rule with a few intervals. Let's take n=2 intervals: points at 0, π/2, π. The function values are f(0)=cos(1)≈0.5403, f(π/2)=0, f(π)=cos(π -1)≈-0.5403. The trapezoidal approximation would be (π/4)[f(0) + 2f(π/2) + f(π)] = (π/4)(0.5403 + 0 -0.5403) = 0. So even with two intervals, it's zero. If I take more points, like n=4, the same symmetry would lead to cancellation. So the integral is indeed zero.

Therefore, the exact answer is 0, and the numerical approximation is also 0.0000000000.
</think>

{"answer": "0", "numerical_answer": "0.0000000000"}