<think>
Okay, let's tackle this integral step by step. The problem is to compute the definite integral from 0 to 7 of the expression ∛(√(x² + 1) + x) minus ∛(√(x² + 1) - x) dx. Hmm, that looks a bit intimidating at first glance, but maybe there's a substitution that can simplify things.

First, let me write down the integral again to get a clear view:

∫₀⁷ [∛(√(x² + 1) + x) - ∛(√(x² + 1) - x)] dx

I need to find an antiderivative for this expression. The presence of √(x² + 1) suggests that hyperbolic trigonometric substitutions might be useful here, or perhaps some algebraic manipulation to simplify the cube roots.

Let me consider the terms inside the cube roots. Let's denote:

A = ∛(√(x² + 1) + x)
B = ∛(√(x² + 1) - x)

So the integrand is A - B. Maybe if I can find a relationship between A and B, or express them in terms of a variable substitution, that would help.

Let me try to find A * B. Let's compute A³ and B³ first.

A³ = √(x² + 1) + x
B³ = √(x² + 1) - x

Multiplying A³ and B³:

A³ * B³ = (√(x² + 1) + x)(√(x² + 1) - x) = (√(x² + 1))² - x² = (x² + 1) - x² = 1

So, A³ * B³ = 1, which implies that (A*B)³ = 1. Therefore, A*B = 1, assuming A and B are real numbers (which they are here). So, A*B = 1. That's a useful relationship.

Now, if A*B = 1, then B = 1/A. So the integrand becomes A - 1/A. Let's set t = A - 1/A. Then, maybe we can find a differential equation or some relation involving t and x.

Alternatively, let's try to express A - B in terms of t. Since B = 1/A, then A - B = A - 1/A. Let's denote t = A - 1/A. Then, t = A - 1/A. Let's cube both sides to see if that helps:

t³ = (A - 1/A)³ = A³ - 3A*(1/A)*(A - 1/A) - (1/A)³

Wait, expanding (a - b)³ = a³ - 3a²b + 3ab² - b³. So:

t³ = A³ - 3A²*(1/A) + 3A*(1/A)² - (1/A)³
= A³ - 3A + 3*(1/A) - (1/A³)

But we know that A³ = √(x² + 1) + x and 1/A³ = B³ = √(x² + 1) - x. So substituting:

t³ = (√(x² + 1) + x) - 3A + 3*(1/A) - (√(x² + 1) - x)
Simplify the terms:

= √(x² + 1) + x - 3A + 3*(1/A) - √(x² + 1) + x
= 2x - 3A + 3*(1/A)

But since t = A - 1/A, then 3*(1/A) = 3*(A - t)/A? Wait, maybe this isn't the right path. Let me check again.

Alternatively, since A³ - (1/A³) = [√(x² +1) + x] - [√(x² +1) - x] = 2x. So:

t³ = (A³ - 1/A³) - 3(A - 1/A) = 2x - 3t

Therefore, t³ + 3t = 2x

So we have t³ + 3t = 2x. That's a key equation. Let me write that:

t³ + 3t = 2x

So, if we can express x in terms of t, maybe we can find a substitution. Let's solve for x:

x = (t³ + 3t)/2

Now, if we can express dx in terms of dt, then we can change variables from x to t. Let's compute dx/dt:

dx/dt = (3t² + 3)/2 = (3/2)(t² + 1)

So, dx = (3/2)(t² + 1) dt

Now, the original integral is ∫(A - B) dx = ∫t dx. Since t = A - B, and we have:

Integral = ∫ t * dx = ∫ t * (3/2)(t² + 1) dt

So, we need to express the integral in terms of t. But we also need to adjust the limits of integration. When x is 0, what is t? And when x is 7, what is t?

Let's compute the limits. When x = 0:

Compute t at x=0:

t = A - B = ∛(√(0 +1) +0) - ∛(√(0 +1) -0) = ∛1 - ∛1 = 1 -1 = 0

So, when x=0, t=0.

When x=7:

Compute t at x=7:

t = ∛(√(7² +1) +7) - ∛(√(7² +1) -7)

First, compute √(49 +1) = √50 = 5√2 ≈7.0710678...

So, √50 +7 ≈5√2 +7, and √50 -7 ≈5√2 -7. Let's compute these:

But 5√2 ≈7.0710678, so √50 -7 ≈0.0710678. So, the cube roots:

A = ∛(5√2 +7), B = ∛(5√2 -7)

But perhaps there's a way to compute t at x=7. Let's see. Let me compute t = A - B. Let's compute A³ and B³:

A³ = 5√2 +7, B³ =5√2 -7

So, t = A - B. Let's compute t³ +3t =2x. Wait, from earlier, we have t³ +3t =2x. So, when x=7, t³ +3t =14. So, we need to find t such that t³ +3t -14=0. Let's try to solve this equation.

Let me try t=2: 8 +6 -14=0. Yes! t=2: 8 +6=14, so 14-14=0. So t=2 is the solution. Therefore, when x=7, t=2.

Therefore, the limits of integration in terms of t are from t=0 to t=2.

So, the integral becomes:

Integral = ∫ from t=0 to t=2 of t * (3/2)(t² +1) dt

Let's compute this integral:

First, factor out the constants:

(3/2) ∫₀² t(t² +1) dt

Multiply t into the parentheses:

(3/2) ∫₀² (t³ + t) dt

Integrate term by term:

Integral of t³ is t⁴/4, integral of t is t²/2. So:

(3/2)[ (t⁴/4 + t²/2) ] from 0 to 2

Compute at upper limit t=2:

(2⁴)/4 + (2²)/2 = 16/4 +4/2 =4 +2=6

At lower limit t=0:

0 +0=0

So, the integral is (3/2)(6 -0) = (3/2)*6=9

So, the exact value of the integral is 9.

Wait, that's surprisingly simple. Let me verify this again to make sure I didn't make a mistake.

So, substitution steps:

1. Let t = A - B, where A and B are the cube roots.

2. Found that t³ +3t =2x.

3. Expressed x in terms of t, then dx in terms of dt.

4. Changed the limits: x=0 gives t=0, x=7 gives t=2.

5. Transformed the integral into (3/2) ∫₀² (t³ + t) dt, which evaluates to 9.

That seems correct. Let me check the substitution again. The integrand is t, and dx is (3/2)(t² +1)dt. So, t*(3/2)(t² +1)dt. Then integrating from 0 to 2. Yes.

Calculating the integral:

∫₀² (t³ + t) dt = [t⁴/4 + t²/2]₀² = (16/4 +4/2) -0 =4 +2=6. Multiply by 3/2: 6*(3/2)=9. Correct.

So the exact answer is 9. The numerical approximation is 9.0000000000.

But wait, the problem says to provide a numerical approximation rounded to 10 decimal places. Since the exact answer is 9, the numerical approximation is exactly 9.0000000000.

But let me confirm once more. Maybe there's a mistake in substitution steps.

Wait, when we set t = A - B, and found that t³ +3t =2x. Then, when x=7, t=2. Then, the integral becomes 9. That seems correct.

Alternatively, maybe check with a numerical approximation. Let's compute the integral numerically for x from 0 to7 and see if it's approximately 9.

But since the analytical solution gives exactly 9, and the steps seem correct, I think the answer is correct.

Therefore, the exact answer is 9, and the numerical approximation is 9.0000000000.
</think>

{"answer": "9", "numerical_answer": "9.0000000000"}