<think>
Okay, so I need to compute the definite integral from 0 to π of sec(x) times the natural logarithm of (1 plus cos(x)/3). Let me start by writing that down:

∫₀^π sec(x) ln(1 + (cos x)/3) dx

Hmm, sec(x) is 1/cos(x), so maybe I can simplify the integrand first. Let me rewrite the integral:

∫₀^π [ln(1 + (cos x)/3)] / cos(x) dx

Hmm, that might not immediately help. Let me think about substitution or integration by parts. Since there's a logarithm, integration by parts might be a good approach. Let me recall that integration by parts formula: ∫u dv = uv - ∫v du.

Let me set u = ln(1 + (cos x)/3), which would make du = [ ( -sin x / 3 ) / (1 + cos x /3 ) ] dx. Wait, let me compute that derivative properly. The derivative of ln(1 + (cos x)/3) with respect to x is [ ( -sin x / 3 ) / (1 + cos x /3 ) ]? Wait, no. Let's do it step by step.

If u = ln(1 + (cos x)/3), then du/dx = [ derivative of the argument ] / (1 + (cos x)/3 )

The derivative of 1 + (cos x)/3 is -sin x / 3. So:

du = [ -sin x / 3 ] / (1 + cos x /3 ) dx

So du = [ -sin x / (3 + cos x) ] dx

Okay, and then dv would be sec x dx, right? Because the integrand is u dv. So dv = sec x dx. Then v is the integral of sec x dx, which is ln |sec x + tan x| + C. But since we're dealing with definite integrals from 0 to π, maybe we can handle the constants later.

So applying integration by parts:

uv | from 0 to π - ∫₀^π v du

So first term: [ ln(1 + cos x /3 ) * ln |sec x + tan x| ] evaluated from 0 to π minus the integral of v times du.

But let's check the first term. At x = π, cos π = -1, so 1 + (-1)/3 = 2/3. So ln(2/3). And sec π is 1/cos π = -1, tan π is 0. So ln |sec π + tan π| = ln | -1 + 0 | = ln 1 = 0. Wait, ln(1) is 0. So the upper limit term is ln(2/3) * 0 = 0.

At x = 0, cos 0 = 1, so 1 + 1/3 = 4/3. ln(4/3). sec 0 = 1, tan 0 = 0. So ln |1 + 0| = ln 1 = 0. So the first term is 0 - 0 = 0. So the entire first part of integration by parts is zero. So now we have:

- ∫₀^π v du

Which is - ∫₀^π [ ln |sec x + tan x| ] * [ -sin x / (3 + cos x) ] dx

Simplify the negatives: the two negatives make a positive, so:

∫₀^π [ ln(sec x + tan x) ] * [ sin x / (3 + cos x) ] dx

Hmm, okay. Now, this integral seems more complicated. Let me see if I can simplify this. Let's note that ln(sec x + tan x) is actually equal to the inverse hyperbolic functions? Wait, actually, the integral of sec x is ln |sec x + tan x|, which is a standard result. But here, we have this term multiplied by sin x / (3 + cos x). Hmm.

Alternatively, maybe there's a substitution here. Let me consider substituting t = cos x. Then dt = -sin x dx. Let's see. Let me try that.

Let t = cos x, so when x=0, t=1; x=π, t=-1. Then dt = -sin x dx, so sin x dx = -dt. Then the integral becomes:

∫₀^π [ ln(sec x + tan x) ] * [ sin x / (3 + cos x) ] dx = ∫ from t=1 to t=-1 [ ln(sec x + tan x) ] * [ (-dt) / (3 + t) ]

But we need to express ln(sec x + tan x) in terms of t. Let's see. Since t = cos x, then sec x = 1/t, and tan x = sqrt(1 - t²)/t, but wait, in terms of t, x is between 0 and π, so sin x is non-negative, so tan x = sin x / cos x = sqrt(1 - t²)/t. But when x is in (π/2, π), cos x is negative, so t is negative, and tan x is negative. Hmm, but sqrt(1 - t²) is positive, so tan x would be negative. So maybe tan x = -sqrt(1 - t²)/t when t is negative? Wait, let's check.

If t = cos x, then sin x = sqrt(1 - t²) when x is in [0, π/2], and sin x is still positive in [π/2, π], but cos x is negative there. So tan x = sin x / cos x = sqrt(1 - t²)/t) when t is positive, and sqrt(1 - t²)/t when t is negative, which would be negative. So tan x = sqrt(1 - t²)/t, but with t's sign. So tan x = sqrt(1 - t²)/t, but since t can be negative, that's equivalent to tan x = sin x / t, but sin x is sqrt(1 - t²). Hmm, maybe it's better to write tan x + sec x.

Wait, sec x + tan x = (1 + sin x)/cos x. Let me verify:

sec x + tan x = 1/cos x + sin x / cos x = (1 + sin x)/cos x. Yes. So ln(sec x + tan x) = ln( (1 + sin x)/cos x ) = ln(1 + sin x) - ln(cos x). But maybe that's not helpful. Alternatively, perhaps we can express (1 + sin x)/cos x in terms of t.

Since t = cos x, sin x = sqrt(1 - t²). So (1 + sin x)/cos x = (1 + sqrt(1 - t²))/t. So ln( (1 + sqrt(1 - t²))/t ). Hmm, that might be complicated. Let me write that:

ln( (1 + sqrt(1 - t²)) / t )

So the integral becomes:

∫ from t=1 to t=-1 [ ln( (1 + sqrt(1 - t²)) / t ) ] * [ -dt / (3 + t) ]

But integrating from 1 to -1 with a -dt, so changing the limits to from -1 to 1 and removing the negative sign:

∫ from t=-1 to t=1 [ ln( (1 + sqrt(1 - t²)) / t ) ] * [ dt / (3 + t) ]

Hmm, this seems complicated. Maybe there's a symmetry here. Let's check if the integrand is even or odd. Let me substitute t → -t. Let me see:

If we let t = -u, then when t = -1, u=1; t=1, u=-1. Then dt = -du. The integral becomes:

∫ from u=1 to u=-1 [ ln( (1 + sqrt(1 - u²)) / (-u) ) ] * [ -du / (3 - u) ]

Hmm, this is getting messy. Maybe not helpful. Alternatively, perhaps split the integral into two parts: from -1 to 0 and 0 to 1? Not sure. Alternatively, maybe consider expanding the logarithm.

Wait, the integrand is [ ln(1 + sqrt(1 - t²)) - ln t ] / (3 + t). So split the integral into two parts:

∫ [ ln(1 + sqrt(1 - t²)) / (3 + t) ] dt - ∫ [ ln t / (3 + t) ] dt from t=-1 to 1.

But integrating from -1 to 1. The second integral, ∫ ln t / (3 + t) dt from -1 to 1. Wait, ln t is only defined for t > 0, so from 0 to 1, but the original substitution t = cos x, so t ranges from 1 to -1. But when t is negative, ln t is not real. Wait, but in the original integral, when x is in (π/2, π), t = cos x is negative, but ln(sec x + tan x) is still real? Let's check.

At x = π/2, sec x is undefined, but the original integral is from 0 to π, so we have to be careful at x=π/2. But maybe the integral is still convergent. Wait, sec x is 1/cos x, which goes to infinity at x=π/2, but the original integrand is sec x ln(1 + cos x /3). At x approaching π/2, cos x approaches 0, so ln(1 + cos x /3) approaches ln(1 + 0) = 0. So the integrand becomes (1/cos x) * (cos x /3 + ...) ~ (1/cos x)(cos x /3) = 1/3, so the integrand approaches 1/3, which is finite. So the integral is convergent at x=π/2.

But back to the substitution. When t is negative, ln t is not real, but in the original expression, ln(sec x + tan x) when x is in (π/2, π), let's see:

sec x + tan x = 1/cos x + sin x / cos x = (1 + sin x)/cos x. When x is in (π/2, π), cos x is negative, and sin x is positive. So (1 + sin x)/cos x is (positive + positive)/negative. Wait, 1 + sin x is always positive since sin x >= -1. So if x is in (π/2, π), cos x is negative, so (1 + sin x)/cos x is negative. Therefore, ln(sec x + tan x) is ln of a negative number, which is complex. But the original integral is supposed to be real. Hmm, this suggests that there might be an issue with the integration by parts step. Wait, but the original integrand is real for all x in [0, π], except at x=π/2 where sec x is undefined. Wait, but ln(1 + cos x /3) is real as long as 1 + cos x /3 > 0. Since cos x ranges from -1 to 1, 1 + cos x /3 ranges from 1 - 1/3 = 2/3 to 1 + 1/3 = 4/3. So the argument of the logarithm is always positive, so ln is real. So the original integrand is real everywhere except at x=π/2, but as we saw, the integrand approaches 1/3 there, so it's a removable discontinuity. So the integral is real.

But when we did substitution t = cos x, and expressed ln(sec x + tan x) in terms of t, we ended up with ln( (1 + sqrt(1 - t²))/t ). However, when t is negative (i.e., x in (π/2, π)), then (1 + sqrt(1 - t²))/t is (positive)/negative, so the argument of ln is negative, which would make the logarithm complex. But the original expression ln(sec x + tan x) is real numbers. Wait, but in reality, when x is in (π/2, π), sec x + tan x is negative, so ln(sec x + tan x) would be complex. But the original integral is real. So this suggests that there's a problem with the integration by parts approach? Wait, but the original integral is real, but after integration by parts, we have an integral that might involve complex numbers. That can't be. So perhaps there's a mistake in the substitution or in the integration by parts.

Wait, maybe I made a mistake in the substitution. Let me check again. When x is in (π/2, π), cos x is negative, so t = cos x is negative. Then sec x + tan x = 1/cos x + sin x / cos x = (1 + sin x)/cos x. Since sin x is positive in (π/2, π), and cos x is negative, so (1 + sin x)/cos x is negative. Therefore, ln(sec x + tan x) is ln of a negative number, which is complex. But the original integral is real, so this suggests that the integration by parts is leading us into complex numbers, which is not desired. Therefore, perhaps integration by parts is not the right approach here, or maybe we need to handle the logarithm of a negative number carefully.

Alternatively, maybe there's a different substitution or method. Let me think. The original integral is ∫₀^π sec x ln(1 + cos x /3) dx. Let me consider another substitution. Let me set t = sin x. Wait, but then dt = cos x dx, which might not help. Alternatively, maybe expand the logarithm into a series.

Since the logarithm can be expanded as a power series. Let me recall that ln(1 + y) = Σ_{n=1}^∞ (-1)^{n+1} y^n / n for |y| < 1. Here, y = cos x /3. The maximum value of cos x is 1, so |y| <= 1/3 < 1, so the series converges for all x. Therefore, we can write:

ln(1 + cos x /3) = Σ_{n=1}^∞ (-1)^{n+1} (cos x)^n / (3^n n)

Then, the integral becomes:

∫₀^π sec x * Σ_{n=1}^∞ (-1)^{n+1} (cos x)^n / (3^n n) dx

But sec x = 1 / cos x, so multiplying by sec x gives:

Σ_{n=1}^∞ (-1)^{n+1} / (3^n n) ∫₀^π (cos x)^{n-1} dx

So the integral simplifies to a sum over n of terms involving ∫₀^π (cos x)^{n-1} dx.

Let me write that:

Integral = Σ_{n=1}^∞ [ (-1)^{n+1} / (3^n n) ] * ∫₀^π (cos x)^{n-1} dx

Now, the integral of (cos x)^{k} dx from 0 to π is a standard integral. For integer k >= 0, the integral ∫₀^π (cos x)^k dx is known. For even k, it's 2^{1 - k} π (k-1 choose k/2), and for odd k, it's 0. Wait, let me recall the exact formula.

The integral ∫₀^{2π} (cos x)^n dx = 2π * (1/2^n) * C(n, floor(n/2)) ) when n is even, and 0 when n is odd. But here, the integral is from 0 to π. So for even exponents, the integral from 0 to π is half of the integral from 0 to 2π. So for even k, ∫₀^π (cos x)^k dx = π * (1/2^{k}) * C(k, k/2). For odd k, it's 0.

But in our case, the exponent is n-1. So if n-1 is even, i.e., n is odd, then the integral is non-zero. If n-1 is odd, i.e., n is even, the integral is zero. Therefore, the sum reduces to terms where n is odd. Let me write n = 2m + 1, where m >= 0. Then:

Integral = Σ_{m=0}^∞ [ (-1)^{2m+2} / (3^{2m+1} (2m+1)) ] * ∫₀^π (cos x)^{2m} dx

Simplify (-1)^{2m+2} = (-1)^{2m} * (-1)^2 = 1 * 1 = 1. So:

Integral = Σ_{m=0}^∞ [ 1 / (3^{2m+1} (2m+1)) ] * [ π * (1/2^{2m}) * C(2m, m) ]

Because for even exponent 2m, the integral is π * (1/2^{2m}) * C(2m, m). Therefore:

Integral = π Σ_{m=0}^∞ [ 1 / (3^{2m+1} (2m+1)) ] * [ (1/2^{2m}) * C(2m, m) ]

Simplify the constants:

= π Σ_{m=0}^∞ [ C(2m, m) / (3^{2m+1} (2m+1) 2^{2m}) ) ]

Combine the exponents:

3^{2m+1} = 3 * 9^m, and 2^{2m} = 4^m. So:

= π / 3 Σ_{m=0}^∞ [ C(2m, m) / ( (9 * 4)^m (2m+1) ) ) ]

Wait, 3^{2m} is 9^m, so 3^{2m+1} = 3 * 9^m. So:

3^{2m+1} * 2^{2m} = 3 * (9*4)^m = 3 * 36^m. So:

= π / 3 Σ_{m=0}^∞ [ C(2m, m) / (36^m (2m+1)) ) ]

Hmm, so the sum is Σ_{m=0}^∞ [ C(2m, m) / ( (36)^m (2m+1) ) ]

I need to evaluate this sum. Let me recall that there is a generating function for C(2m, m). The generating function for C(2m, m) x^m is 1 / sqrt(1 - 4x). But here, we have an extra 1/(2m+1) term. Let me think.

Let me denote S = Σ_{m=0}^∞ [ C(2m, m) / ( (36)^m (2m+1) ) ]

Let me write this as S = Σ_{m=0}^∞ [ C(2m, m) / (2m+1) ) * (1/36)^m ]

Let me consider the general series Σ_{m=0}^∞ C(2m, m) x^m / (2m+1). If I can find a closed-form for this series, then I can plug in x = 1/36.

Let me recall that ∫₀^1 t^{2m} dt = 1/(2m+1). So perhaps:

Σ_{m=0}^∞ C(2m, m) x^m}/(2m+1) = Σ_{m=0}^∞ C(2m, m) x^m ∫₀^1 t^{2m} dt = ∫₀^1 Σ_{m=0}^∞ C(2m, m) (x t²)^m dt

Interchange sum and integral (if valid):

= ∫₀^1 [ Σ_{m=0}^∞ C(2m, m) (x t²)^m ] dt

But the generating function Σ_{m=0}^∞ C(2m, m) z^m = 1 / sqrt(1 - 4z). So substituting z = x t²:

= ∫₀^1 1 / sqrt(1 - 4 x t²) dt

Therefore, S = ∫₀^1 1 / sqrt(1 - 4 x t²) dt

So for our case, x = 1/36, so:

S = ∫₀^1 1 / sqrt(1 - 4*(1/36)*t²) dt = ∫₀^1 1 / sqrt(1 - (t²)/9) dt = ∫₀^1 1 / sqrt(1 - (t/3)^2) dt

This is a standard integral. Let me make substitution u = t/3, so t = 3u, dt = 3 du. When t=0, u=0; t=1, u=1/3.

So S = ∫₀^{1/3} 1 / sqrt(1 - u²) * 3 du = 3 [ arcsin u ] from 0 to 1/3 = 3 (arcsin(1/3) - arcsin 0) = 3 arcsin(1/3)

Therefore, the original integral is:

Integral = π / 3 * S = π / 3 * 3 arcsin(1/3) = π arcsin(1/3)

Wait, wait, let's check:

Wait, S = 3 arcsin(1/3), and Integral = π / 3 * S? Wait, no. Wait, the original expression was:

Integral = π / 3 * S, where S = 3 arcsin(1/3). So Integral = π / 3 * 3 arcsin(1/3) = π arcsin(1/3)

Yes. So the integral evaluates to π times arcsin(1/3). But arcsin(1/3) is the same as arctan(1 / sqrt(8)), but maybe we can leave it as arcsin(1/3). Alternatively, we can express it in terms of other inverse trigonometric functions, but perhaps π arcsin(1/3) is the simplest exact form.

Therefore, the exact answer is π arcsin(1/3). Let me verify this result.

Wait, let me check with numerical approximation. Let's compute the numerical value. Let's compute π * arcsin(1/3). First, compute arcsin(1/3) in radians. 1/3 is approximately 0.3333. The arcsin of 1/3 is approximately 0.3398 radians. Then π times that is approximately 3.1416 * 0.3398 ≈ 1.0679. Let me check with numerical integration of the original integral.

Alternatively, let me compute the original integral numerically. Let's approximate ∫₀^π sec x ln(1 + cos x /3) dx. But integrating from 0 to π, but sec x has a singularity at π/2. However, as we saw earlier, the integrand approaches 1/3 at π/2, so it's a removable singularity. So we can numerically integrate.

But since I don't have a calculator here, but I can estimate. Let's see, if the exact answer is π arcsin(1/3), then π * 0.3398 ≈ 1.067. Let me check with another approach. Alternatively, maybe the answer is π times arctan(sqrt(2)/4) or something else. Wait, but let's see.

Wait, arcsin(1/3) is the angle whose sine is 1/3. So the cosine of that angle is sqrt(1 - (1/3)^2) = sqrt(8/9) = 2√2/3. So tan(arcsin(1/3)) = (1/3)/(2√2/3) = 1/(2√2) = √2/4. Therefore, arcsin(1/3) = arctan(√2/4). So the integral can also be written as π arctan(√2/4). But both forms are acceptable. However, the problem says to compute the exact answer, so either π arcsin(1/3) or π arctan(√2/4) would be correct. Let me check which one is simpler.

Alternatively, maybe there's a more simplified form. Let me think. If we consider the integral result, perhaps there's a different representation. But given the steps we took, the series expansion led us to π arcsin(1/3). So that's the exact answer.

Now, let's compute the numerical approximation. Let's compute arcsin(1/3):

arcsin(1/3) ≈ 0.3398369094541219 radians.

Multiply by π:

0.3398369094541219 * π ≈ 1.0676274677542664.

Rounded to 10 decimal places, that's approximately 1.0676274678.

Let me verify this with a numerical integration. Suppose we approximate the integral ∫₀^π sec x ln(1 + cos x /3) dx numerically. Since I can't compute it here, but I can check with substitution. Alternatively, if I use symmetry. Wait, the integrand is not symmetric around π/2. Let me check the original integral:

At x and π - x, cos(π - x) = -cos x. So sec(π - x) = -sec x, and ln(1 + cos(π - x)/3) = ln(1 - cos x /3). So the integrand at x and π - x are -sec x ln(1 - cos x /3). Not sure if that helps. Maybe not.

Alternatively, perhaps use substitution x = π - t. Let me try:

Let I = ∫₀^π sec x ln(1 + cos x /3) dx.

Let x = π - t, so when x=0, t=π; x=π, t=0. dx = -dt. So:

I = ∫π^0 sec(π - t) ln(1 + cos(π - t)/3) (-dt) = ∫₀^π sec(π - t) ln(1 - cos t /3) dt

But sec(π - t) = -sec t. So:

I = ∫₀^π (-sec t) ln(1 - cos t /3) dt = -∫₀^π sec t ln(1 - cos t /3) dt

So we have:

I = -∫₀^π sec t ln(1 - cos t /3) dt

But this is another integral. If we add the original expression for I and this new expression:

I + I = ∫₀^π sec x [ ln(1 + cos x /3) - ln(1 - cos x /3) ] dx

But 2I = ∫₀^π sec x ln( (1 + cos x /3)/(1 - cos x /3) ) dx

Simplify the argument of the log:

(1 + cos x /3)/(1 - cos x /3) = [ (3 + cos x)/3 ] / [ (3 - cos x)/3 ] = (3 + cos x)/(3 - cos x)

So 2I = ∫₀^π sec x ln( (3 + cos x)/(3 - cos x) ) dx

Hmm, not sure if this helps. Maybe another substitution. Let me set u = sin x. Then du = cos x dx. But not sure. Alternatively, expand the logarithm as a series.

Alternatively, note that ln( (3 + cos x)/(3 - cos x) ) = 2 artanh( cos x /3 ), since artanh(z) = (1/2) ln( (1 + z)/(1 - z) ). So:

2I = 2 ∫₀^π sec x artanh( cos x /3 ) dx

So I = ∫₀^π sec x artanh( cos x /3 ) dx

But I don't know if this helps. Maybe not. Let's return to our previous result. We have the exact answer as π arcsin(1/3), and the numerical approximation is approximately 1.0676274678.

Let me check with another approach. Suppose we use the original substitution t = cos x. Then dt = -sin x dx. The original integral is:

I = ∫₀^π sec x ln(1 + cos x /3) dx = ∫₀^π [ ln(1 + cos x /3) ] / cos x dx

Let t = cos x, so when x=0, t=1; x=π, t=-1. Then dt = -sin x dx. But we need to express the integral in terms of t. Note that sin x = sqrt(1 - t²), but in the original integral, we have 1/cos x dx. So:

dx = - dt / sin x = - dt / sqrt(1 - t²)

So the integral becomes:

I = ∫_{1}^{-1} [ ln(1 + t/3) / t ] * [ - dt / sqrt(1 - t²) ]

= ∫_{-1}^{1} [ ln(1 + t/3) / t ] * [ dt / sqrt(1 - t²) ]

This integral is from -1 to 1. Let me split it into two parts: from -1 to 0 and 0 to 1.

But the integrand has a term 1/t, which is problematic at t=0. However, the original integral is convergent there. Let's check near t=0. The integrand is [ ln(1 + t/3) / t ] / sqrt(1 - t²). As t approaches 0, ln(1 + t/3) ~ t/3 - (t/3)^2 /2 + ..., so ln(1 + t/3)/t ~ 1/3 - t/18 + ..., and sqrt(1 - t²) ~ 1 - t²/2. So the integrand ~ (1/3) / 1 = 1/3 as t approaches 0, so the integral is convergent.

But integrating from -1 to 1. Let me consider the integrand for t and -t. Let me substitute u = -t in the integral from -1 to 0:

When t = -u, dt = -du. The integral from -1 to 0 becomes:

∫_{u=1}^{0} [ ln(1 - u/3) / (-u) ] / sqrt(1 - u²) (-du) = ∫₀^1 [ ln(1 - u/3) / (-u) ] / sqrt(1 - u²) du

= ∫₀^1 [ -ln(1 - u/3) / u ] / sqrt(1 - u²) du

So the total integral I is:

∫₀^1 [ ln(1 + u/3) / u ] / sqrt(1 - u²) du + ∫₀^1 [ -ln(1 - u/3) / u ] / sqrt(1 - u²) du

= ∫₀^1 [ ln(1 + u/3) - ln(1 - u/3) ] / (u sqrt(1 - u²)) du

= ∫₀^1 [ ln( (1 + u/3)/(1 - u/3) ) ] / (u sqrt(1 - u²)) du

Again, this is similar to the previous expression. Using the identity for artanh:

ln( (1 + u/3)/(1 - u/3) ) = 2 artanh(u/3)

So:

I = ∫₀^1 [ 2 artanh(u/3) ] / (u sqrt(1 - u²)) du

= 2 ∫₀^1 artanh(u/3) / (u sqrt(1 - u²)) du

This seems complicated, but perhaps expanding artanh(u/3) as a series. Recall that artanh(z) = Σ_{k=0}^∞ z^{2k+1}/(2k+1) for |z| < 1. Here, z = u/3, and u is in [0,1], so |z| <= 1/3 < 1, so the series converges.

So:

artanh(u/3) = Σ_{k=0}^∞ (u/3)^{2k+1} / (2k+1)

Therefore:

I = 2 ∫₀^1 [ Σ_{k=0}^∞ (u^{2k+1} / 3^{2k+1} (2k+1)) ] / (u sqrt(1 - u²)) du

= 2 Σ_{k=0}^∞ [ 1 / (3^{2k+1} (2k+1)) ] ∫₀^1 u^{2k} / sqrt(1 - u²) du

Let me compute the integral ∫₀^1 u^{2k} / sqrt(1 - u²) du. Let me substitute v = u², so dv = 2u du, but not sure. Alternatively, use substitution t = u². Let me set t = u², then dt = 2u du, but the integral is u^{2k} / sqrt(1 - u²) du. Let me try substitution t = u². Then u = sqrt(t), du = (1/(2 sqrt(t))) dt. So:

∫₀^1 u^{2k} / sqrt(1 - u²) du = ∫₀^1 t^k / sqrt(1 - t) * (1/(2 sqrt(t))) dt = (1/2) ∫₀^1 t^{k - 1/2} (1 - t)^{-1/2} dt

This is the Beta function B(k + 1/2, 1/2) / 2. The Beta function B(m, n) = Γ(m)Γ(n)/Γ(m + n). So:

B(k + 1/2, 1/2) = Γ(k + 1/2)Γ(1/2)/Γ(k + 1)

We know that Γ(1/2) = sqrt(π), Γ(k + 1) = k!, and Γ(k + 1/2) = (2k)! sqrt(π) / 4^k k!.

Therefore:

B(k + 1/2, 1/2) = [ (2k)! sqrt(π) / 4^k k! ) ] * sqrt(π) / k! )

Wait, let me check:

Γ(k + 1/2) = (2k)! sqrt(π) / (4^k k! )

So:

B(k + 1/2, 1/2) = [ (2k)! sqrt(π) / 4^k k! ) ] * sqrt(π) / Γ(k + 1)

But Γ(k + 1) = k!.

So:

B(k + 1/2, 1/2) = (2k)! π / (4^k (k!)^2 )

Therefore, the integral becomes:

(1/2) * (2k)! π / (4^k (k!)^2 )

So:

∫₀^1 u^{2k} / sqrt(1 - u²) du = (1/2) * (2k)! π / (4^k (k!)^2 )

Therefore, the integral I becomes:

I = 2 Σ_{k=0}^∞ [ 1 / (3^{2k+1} (2k+1)) ] * [ (1/2) * (2k)! π / (4^k (k!)^2 ) ]

Simplify:

= 2 * (1/2) π Σ_{k=0}^∞ [ (2k)! / (4^k (k!)^2 ) ] / (3^{2k+1} (2k+1) )

= π Σ_{k=0}^∞ [ (2k)! / (4^k (k!)^2 ) ] / (3^{2k+1} (2k+1) )

Simplify the terms:

3^{2k+1} = 3 * 9^k, and 4^k = (2^2)^k = 2^{2k}. So:

= π / 3 Σ_{k=0}^∞ [ (2k)! / ( (4 * 9)^k (k!)^2 ) ] / (2k+1 )

4 * 9 = 36, so:

= π / 3 Σ_{k=0}^∞ [ (2k)! / (36^k (k!)^2 ) ] / (2k+1 )

But (2k)! / (k!)^2 is the central binomial coefficient C(2k, k). So:

= π / 3 Σ_{k=0}^∞ [ C(2k, k) / 36^k ] / (2k+1 )

Which is the same series we had before, leading to S = 3 arcsin(1/3), so I = π arcsin(1/3). Therefore, this confirms the result.

Thus, the exact answer is π arcsin(1/3), and the numerical approximation is approximately 1.0676274678 when rounded to 10 decimal places.
</think>

{"answer": "\\pi \\arcsin\\left(\\frac{1}{3}\\right)", "numerical_answer": "1.0676274678"}