To compute the definite integral \(\int_{0}^{1} \arcsin(x) \arccos(x) \, dx\), we can follow these steps:

### Step 1: Simplify the Integrand
First, observe that \(\arcsin(x) + \arccos(x) = \frac{\pi}{2}\) for all \(x \in [-1, 1]\). Therefore, we can express \(\arccos(x)\) as:
\[
\arccos(x) = \frac{\pi}{2} - \arcsin(x)
\]
Substituting this into the integrand:
\[
\arcsin(x) \arccos(x) = \arcsin(x) \left(\frac{\pi}{2} - \arcsin(x)\right) = \frac{\pi}{2} \arcsin(x) - \arcsin^2(x)
\]
So the integral becomes:
\[
\int_{0}^{1} \arcsin(x) \arccos(x) \, dx = \frac{\pi}{2} \int_{0}^{1} \arcsin(x) \, dx - \int_{0}^{1} \arcsin^2(x) \, dx
\]

### Step 2: Compute \(\int_{0}^{1} \arcsin(x) \, dx\)
Using integration by parts:
\[
\int \arcsin(x) \, dx = x \arcsin(x) + \sqrt{1 - x^2} + C
\]
Evaluating from 0 to 1:
\[
\int_{0}^{1} \arcsin(x) \, dx = \left[ x \arcsin(x) + \sqrt{1 - x^2} \right]_{0}^{1} = \left(1 \cdot \frac{\pi}{2} + 0\right) - \left(0 + 1\right) = \frac{\pi}{2} - 1
\]

### Step 3: Compute \(\int_{0}^{1} \arcsin^2(x) \, dx\)
Using integration by parts:
Let \(u = \arcsin^2(x)\), \(dv = dx\). Then:
\[
du = \frac{2 \arcsin(x)}{\sqrt{1 - x^2}} \, dx, \quad v = x
\]
So:
\[
\int \arcsin^2(x) \, dx = x \arcsin^2(x) - \int \frac{2x \arcsin(x)}{\sqrt{1 - x^2}} \, dx
\]
For the remaining integral, let \(w = \arcsin(x)\), then \(dw = \frac{1}{\sqrt{1 - x^2}} \, dx\):
\[
\int \frac{2x \arcsin(x)}{\sqrt{1 - x^2}} \, dx = 2 \int w \sin(w) \, dw
\]
Using integration by parts again:
\[
\int w \sin(w) \, dw = -w \cos(w) + \int \cos(w) \, dw = -w \cos(w) + \sin(w) + C
\]
Substituting back:
\[
\int \frac{2x \arcsin(x)}{\sqrt{1 - x^2}} \, dx = 2 \left( -\arcsin(x) \sqrt{1 - x^2} + x \right) + C
\]
Thus:
\[
\int \arcsin^2(x) \, dx = x \arcsin^2(x) + 2 \arcsin(x) \sqrt{1 - x^2} - 2x + C
\]
Evaluating from 0 to 1:
\[
\int_{0}^{1} \arcsin^2(x) \, dx = \left(1 \cdot \left(\frac{\pi}{2}\right)^2 + 2 \cdot \frac{\pi}{2} \cdot 0 - 2 \cdot 1\right) - \left(0 + 0 - 0\right) = \frac{\pi^2}{4} - 2
\]

### Step 4: Combine the Results
Now, substitute the results from Step 2 and Step 3 into the original expression:
\[
\int_{0}^{1} \arcsin(x) \arccos(x) \, dx = \frac{\pi}{2} \left(\frac{\pi}{2} - 1\right) - \left(\frac{\pi^2}{4} - 2\right) = \frac{\pi^2}{4} - \frac{\pi}{2} - \frac{\pi^2}{4} + 2 = 2 - \frac{\pi}{2}
\]

### Step 5: Numerical Approximation
The exact answer is \(2 - \frac{\pi}{2}\). Numerically:
\[
2 - \frac{\pi}{2} \approx 2 - 1.5707963268 = 0.4292036732
\]

### Final Answer
```json
{"answer": "2 - \\frac{\\pi}{2}", "numerical_answer": "0.4292036732"}
```