To solve the definite integral \(\int\limits_{0}^{2} H_{3}\left(\sqrt{x(2-x)}\right) dx\), where \(H_{3}(y)\) is the third Hermite polynomial, we follow these steps:

### Step 1: Recall the Definition of the Hermite Polynomial
The third Hermite polynomial is given by:
\[
H_{3}(y) = 8y^{3} - 12y
\]

### Step 2: Substitute the Argument
The argument of the Hermite polynomial in the integral is \(y = \sqrt{x(2-x)}\). Substituting this into \(H_{3}(y)\):
\[
H_{3}\left(\sqrt{x(2-x)}\right) = 8\left(\sqrt{x(2-x)}\right)^{3} - 12\sqrt{x(2-x)}
\]
\[
= 8(x(2-x))^{3/2} - 12\sqrt{x(2-x)}
\]

### Step 3: Simplify the Integral
The integral becomes:
\[
\int_{0}^{2} \left[8(x(2-x))^{3/2} - 12\sqrt{x(2-x)}\right] dx
\]
\[
= 8 \int_{0}^{2} (x(2-x))^{3/2} dx - 12 \int_{0}^{2} \sqrt{x(2-x)} dx
\]

### Step 4: Evaluate the Integrals
#### Integral 1: \(\int_{0}^{2} (x(2-x))^{3/2} dx\)
Let \(x = 1 + \sin \theta\), then \(dx = \cos \theta d\theta\), and the limits change from \(\theta = -\pi/2\) to \(\theta = \pi/2\). The integrand becomes:
\[
(x(2-x))^{3/2} = (1 - \sin^{2}\theta)^{3/2} = \cos^{3}\theta
\]
Thus:
\[
\int_{-\pi/2}^{\pi/2} \cos^{4}\theta d\theta
\]
Using the identity \(\cos^{2}\theta = \frac{1 + \cos 2\theta}{2}\):
\[
\cos^{4}\theta = \left(\frac{1 + \cos 2\theta}{2}\right)^{2} = \frac{1 + 2\cos 2\theta + \cos^{2}2\theta}{4}
\]
Integrating term by term:
\[
\int_{-\pi/2}^{\pi/2} \cos^{4}\theta d\theta = \frac{3\pi}{8}
\]
So:
\[
8 \int_{0}^{2} (x(2-x))^{3/2} dx = 8 \cdot \frac{3\pi}{8} = 3\pi
\]

#### Integral 2: \(\int_{0}^{2} \sqrt{x(2-x)} dx\)
Similarly, using the substitution \(x = 1 + \sin \theta\):
\[
\sqrt{x(2-x)} = \cos \theta
\]
\[
\int_{-\pi/2}^{\pi/2} \cos^{2}\theta d\theta = \frac{\pi}{2}
\]
Thus:
\[
-12 \int_{0}^{2} \sqrt{x(2-x)} dx = -12 \cdot \frac{\pi}{2} = -6\pi
\]

### Step 5: Combine the Results
\[
3\pi - 6\pi = -3\pi
\]

### Step 6: Numerical Approximation
\[
-3\pi \approx -9.4247779608
\]

### Final Answer
```json
{"answer": "-3\\pi", "numerical_answer": "-9.4247779608"}
```