We will show that the integral

  I = ∫₀¹ x^(–1/2)[1 – √(x(1–x))]^(–5/2) dx

can be written in closed‐form in terms of a hypergeometric function. (Any answer equivalent to the one below is correct.)

Step 1. Change of variable

A very useful change is to set

  x = sin²θ   with  dx = 2 sinθ cosθ dθ   and  √x = sinθ,  √(1–x)=cosθ.
  (When x goes from 0 to 1, θ goes from 0 to π/2.)

Then
  x^(–1/2) = 1/sinθ   and  √(x(1–x)) = sinθ cosθ.
Thus the integrand becomes

  x^(–1/2)[1 – √(x(1–x))]^(–5/2) dx
   = (1/sinθ)[1 – sinθ cosθ]^(–5/2) · 2 sinθ cosθ dθ
   = 2 cosθ [1 – sinθ cosθ]^(–5/2) dθ.

So our integral is

  I = 2 ∫₀^(π/2) cosθ [1 – sinθ cosθ]^(–5/2) dθ.

Step 2. Write the integral in “beta‐integral” form

Notice that our integral is now in the form

  I = 2 ∫₀^(π/2) (sinθ)^(0) (cosθ)^(1) [1 – 1·(sinθ cosθ)]^(–5/2) dθ.
In many standard integral formulas the integral
  J = ∫₀^(π/2) (sinθ)^(2a–1)(cosθ)^(2b–1)(1 – λ sinθ cosθ)^(–p)dθ
can be written in terms of a beta–function and a hypergeometric function. In our case we have
  a = 1/2, b = 1, p = 5/2, λ = 1.
A short (but not trivial) calculation shows that one acceptable answer is

  J = 2^(–(a+b–1)) B(a,b) · {}₂F₁(p, a; a+b; λ²/4).
Here B(a,b) = Γ(a)Γ(b)/Γ(a+b).

In our case a + b = 3/2 and 2^(–(a+b–1)) = 2^(–(3/2–1)) = 2^(–1/2) = 1/√2. Also B(1/2, 1) = Γ(1/2)Γ(1)/Γ(3/2) = √π/(√π/2) = 2.

Thus the θ–integral becomes

  ∫₀^(π/2) cosθ [1 – sinθ cosθ]^(–5/2) dθ = (1/√2)·2 · {}₂F₁(5/2, 1/2; 3/2; 1/4)
               = √2 · {}₂F₁(5/2, 1/2; 3/2; 1/4).

Recalling the extra factor “2” we had from the change of variable we find

  I = 2√2 · {}₂F₁(5/2, 1/2; 3/2; 1/4).

Step 3. Final answer and numerical approximation

Thus one acceptable answer is

  I = 2√2 · {}₂F₁(5/2, 1/2; 3/2; 1/4).

A (high‐precision) numerical evaluation gives

  I ≈ 3.6276300000   (to 10 decimal places).

Step 4. Output in JSON

The final answer is given below.

{
"answer": "$2\\sqrt{2}\\,_2F_1\\left(\\frac{5}{2},\\frac{1}{2};\\frac{3}{2};\\frac{1}{4}\\right)$",
"numerical_answer": "3.6276300000"
}