Let's solve the integral step by step:

\[
I = \int_{0}^{1} \frac{x^{3} + x + 1}{3x^{2} - 3x + 4} \, dx
\]

**Step 1: Polynomial Long Division**

Notice that the degree of the numerator (3) is higher than that of the denominator (2). Let's perform polynomial division:

Divide \(x^3\) by \(3x^2\):

- First term: \(\frac{1}{3}x\)
- Multiply: \(\frac{1}{3}x \cdot (3x^2-3x+4) = x^3 - x^2 + \frac{4}{3}x\)
- Subtract from numerator:

\[
x^3 + x + 1 - (x^3 - x^2 + \frac{4}{3}x) = x^2 + x + 1 - \frac{4}{3}x = x^2 + x - \frac{4}{3}x + 1 = x^2 - \frac{1}{3}x + 1
\]

Now divide \(x^2\) by \(3x^2\):

- Next term: \(\frac{1}{3}\)
- Multiply: \(\frac{1}{3}(3x^2-3x+4) = x^2 - x + \frac{4}{3}\)
- Subtract:

\[
x^2 - \frac{1}{3}x + 1 - (x^2 - x + \frac{4}{3}) = -\frac{1}{3}x + x - \frac{4}{3} + 1 = \frac{2}{3}x - \frac{1}{3}
\]

So the original fraction can be rewritten as:

\[
\frac{x^{3} + x + 1}{3x^{2} - 3x + 4} = \frac{1}{3}x + \frac{1}{3} + \frac{\frac{2}{3}x - \frac{1}{3}}{3x^2 - 3x + 4}
\]

**Step 2: Split the Integral**

\[
I = \int_{0}^{1} \left( \frac{1}{3}x + \frac{1}{3} \right) dx + \int_{0}^{1} \frac{\frac{2}{3}x - \frac{1}{3}}{3x^2 - 3x + 4} dx
\]
\[
= \frac{1}{3}\int_{0}^{1} x\,dx + \frac{1}{3}\int_{0}^{1} dx + \int_{0}^{1} \frac{2x - 1}{3(3x^2 - 3x + 4)} dx
\]

Let's calculate each part:

a) \(\frac{1}{3}\int_{0}^{1} x\,dx = \frac{1}{3}\left[\frac{1}{2}x^2\right]_{0}^{1} = \frac{1}{3} \cdot \frac{1}{2} = \frac{1}{6}\)

b) \(\frac{1}{3} \int_{0}^{1} dx = \frac{1}{3} [x]_{0}^{1} = \frac{1}{3}\)

c) Focus on:

\[
J = \int_{0}^{1} \frac{2x-1}{3(3x^2 - 3x + 4)} dx
\]

Let's take the 3 outside:

\[
J = \frac{1}{3} \int_{0}^{1} \frac{2x - 1}{3x^2 - 3x + 4} dx
\]

Let \( u = 3x^2 - 3x + 4 \), so:

- \( du = 6x - 3 \)
- Notice \( 2x-1 = \frac{1}{3}(6x - 3) \), so \(2x-1 = \frac{1}{3} du \)

Thus,

\[
J = \frac{1}{3} \int_{x=0}^{x=1} \frac{2x-1}{3x^2 - 3x + 4} dx = \frac{1}{3} \int_{x=0}^{x=1} \frac{1}{3} \frac{du}{u} = \frac{1}{9} \int_{u_0}^{u_1} \frac{du}{u}
\]

Where \( u_0 = 3\cdot 0^2 - 3 \cdot 0 + 4 = 4 \), \( u_1 = 3 \cdot 1^2 - 3 \cdot 1 + 4 = 3-3+4 = 4 \).

So \(u_0 = u_1 = 4\), so:

\[
J = \frac{1}{9} \left[ \ln u \right]_{4}^{4} = \frac{1}{9}(0) = 0
\]

**Step 3: Sum Everything**

So,

\[
I = \frac{1}{6} + \frac{1}{3} + 0 = \frac{1}{6} + \frac{2}{6} = \frac{3}{6} = \frac{1}{2}
\]

**Step 4: Numerical Approximation**

\[
\frac{1}{2} = 0.5
\]

**Final JSON Output:**

{"answer": "\\frac{1}{2}", "numerical_answer": "0.5000000000"}