

To solve the definite integral \(\int_0^\infty \frac{\{x\}^{\lceil x \rceil}}{1+\lceil x \rceil} \, dx\), we proceed as follows:

### Step 1: Analyze the integrand over intervals
The fractional part \(\{x\} = x - \lfloor x \rfloor\) and the ceiling function \(\lceil x \rceil\) are piecewise constant over intervals of the form \([n, n+1)\) for \(n \in \mathbb{N} \cup \{0\}\). Specifically:
- For \(x \in [n, n+1)\), \(\lfloor x \rfloor = n\), so \(\{x\} = x - n\).
- For \(x \in (n, n+1)\) (excluding the integer \(n\)), \(\lceil x \rceil = n+1\) (since the ceiling of a non-integer in \([n, n+1)\) is \(n+1\)).

### Step 2: Split the integral into intervals
The integral over \([0, \infty)\) can be decomposed into a sum of integrals over \([n, n+1)\) for \(n \geq 0\):
\[
\int_0^\infty \frac{\{x\}^{\lceil x \rceil}}{1+\lceil x \rceil} \, dx = \sum_{n=0}^\infty \int_n^{n+1} \frac{(x - n)^{n+1}}{(n+1) + 1} \, dx.
\]
Here, \(\{x\} = x - n\) and \(\lceil x \rceil = n+1\) for \(x \in (n, n+1)\), so the integrand simplifies to \(\frac{(x - n)^{n+1}}{n+2}\).

### Step 3: Evaluate each integral
For each \(n\), substitute \(t = x - n\) (so \(t \in [0, 1)\) and \(dx = dt\)). The integral over \([n, n+1)\) becomes:
\[
\int_n^{n+1} \frac{(x - n)^{n+1}}{n+2} \, dx = \int_0^1 \frac{t^{n+1}}{n+2} \, dt.
\]
Integrating \(t^{n+1}\) over \([0, 1]\) gives:
\[
\int_0^1 t^{n+1} \, dt = \left. \frac{t^{n+2}}{n+2} \right|_0^1 = \frac{1}{n+2}.
\]
Thus, the integral over \([n, n+1)\) simplifies to:
\[
\frac{1}{n+2} \cdot \frac{1}{n+2} = \frac{1}{(n+2)^2}.
\]

### Step 4: Sum the series
The original integral is the sum of these terms over \(n \geq 0\):
\[
\sum_{n=0}^\infty \frac{1}{(n+2)^2}.
\]
Reindexing the series with \(k = n+2\) (so \(k \geq 2\)), we recognize this as:
\[
\sum_{k=2}^\infty \frac{1}{k^2}.
\]
The sum of \(\frac{1}{k^2}\) over all \(k \geq 1\) is \(\frac{\pi^2}{6}\). Subtracting the first term (\(k=1\)) gives:
\[
\sum_{k=2}^\infty \frac{1}{k^2} = \frac{\pi^2}{6} - 1.
\]

### Numerical Approximation
Using \(\pi^2 \approx 9.8696044\), we find:
\[
\frac{\pi^2}{6} - 1 \approx \frac{9.8696044}{6} - 1 \approx 1.6449340868 - 1 = 0.6449340868.
\]

{"answer": "\(\frac{\pi^2}{6} - 1\)", "numerical_answer": "0.6449340868"}