
To solve the definite integral \(\int\limits_0^{2} x^{1 - 3/2}(2 - x)^{1 - 1/2}[1 - 0.5x(2 - x)]^{-1} \, dx\), we proceed as follows:

### Step 1: Simplify the integrand
First, simplify the exponents:
- \(1 - 3/2 = -1/2\), so \(x^{1 - 3/2} = x^{-1/2}\).
- \(1 - 1/2 = 1/2\), so \((2 - x)^{1 - 1/2} = (2 - x)^{1/2}\).

The integrand becomes:
\[
x^{-1/2}(2 - x)^{1/2} \cdot \frac{1}{1 - 0.5x(2 - x)}.
\]

### Step 2: Substitution \(t = x/2\)
Let \(x = 2t\), so \(dx = 2dt\). When \(x = 0\), \(t = 0\); when \(x = 2\), \(t = 1\). Substituting:
- \(x^{-1/2} = (2t)^{-1/2} = 2^{-1/2}t^{-1/2}\),
- \((2 - x)^{1/2} = (2(1 - t))^{1/2} = 2^{1/2}(1 - t)^{1/2}\),
- \(1 - 0.5x(2 - x) = 1 - 2t(1 - t) = 1 - 2t + 2t^2\).

The integral transforms to:
\[
2 \int_0^1 \frac{t^{-1/2}(1 - t)^{1/2}}{1 - 2t + 2t^2} \, dt.
\]

### Step 3: Simplify the denominator
Rewrite \(1 - 2t + 2t^2 = (2t - 1)^2 + 1\). Let \(u = 2t - 1\), so \(t = \frac{u + 1}{2}\) and \(dt = \frac{du}{2}\). When \(t = 0\), \(u = -1\); when \(t = 1\), \(u = 1\). Substituting:
- \(t^{-1/2} = \left(\frac{u + 1}{2}\right)^{-1/2} = 2^{1/2}(u + 1)^{-1/2}\),
- \((1 - t)^{1/2} = \left(\frac{1 - u}{2}\right)^{1/2} = 2^{-1/2}(1 - u)^{1/2}\),
- \(1 - 2t + 2t^2 = u^2 + 1\).

The integral becomes:
\[
2 \int_{-1}^1 \frac{\sqrt{\frac{1 - u}{1 + u}}}{u^2 + 1} \, du.
\]

### Step 4: Substitution \(w = \frac{1 - u}{1 + u}\)
Let \(w = \frac{1 - u}{1 + u}\), so \(u = \frac{1 - w}{1 + w}\) and \(du = -\frac{2}{(1 + w)^2}dw\). When \(u = -1\), \(w \to \infty\); when \(u = 1\), \(w = 0\). The integrand simplifies to:
\[
\sqrt{w} \cdot \frac{(1 + w)^2}{2(1 + w^2)} \cdot \frac{2}{(1 + w)^2} = \frac{\sqrt{w}}{1 + w^2}.
\]

The integral reduces to:
\[
\int_0^\infty \frac{w^{1/2}}{1 + w^2} \, dw.
\]

### Step 5: Evaluate the standard integral
The integral \(\int_0^\infty \frac{w^{s - 1}}{1 + w^a} \, dw = \frac{\pi}{a \sin\left(\frac{\pi s}{a}\right)}\) for \(0 < s < a\). Here, \(s = 3/2\) and \(a = 2\), so:
\[
\int_0^\infty \frac{w^{1/2}}{1 + w^2} \, dw = \frac{\pi}{2 \sin\left(\frac{3\pi}{4}\right)} = \frac{\pi}{\sqrt{2}}.
\]

### Step 6: Combine results
The original integral equals \(2 \cdot \frac{\pi}{\sqrt{2}} = \sqrt{2}\pi\).

### Numerical Approximation
\(\sqrt{2}\pi \approx 4.442882908\).

{"answer": "\(\sqrt{2}\pi\)", "numerical_answer": "4.442882908"}