<think>
Okay, let's tackle this integral: ∫₀² [1/(x(2 - x))] arctan(√(x(2 - x))) dx. Hmm, first, the integrand looks a bit complicated. Let me see if I can simplify it or find a substitution that works.

The expression inside the arctan is √(x(2 - x)). That term x(2 - x) is a quadratic that peaks at x=1, right? It's symmetric around x=1. Maybe symmetry could help here. Let me try substituting t = x - 1 to center the integral around zero. So, let t = x - 1, which means x = t + 1, and when x=0, t=-1; x=2, t=1. Then dx = dt. The integral becomes ∫₋₁¹ [1/((t + 1)(1 - t))] arctan(√((t + 1)(1 - t))) dt. Simplifying the denominator: (t + 1)(1 - t) = 1 - t². So the integrand is [1/(1 - t²)] arctan(√(1 - t²)). That seems a bit better. The limits are symmetric now, from -1 to 1. Maybe the function is even? Let's check. If we replace t with -t, the denominator 1 - t² stays the same, and √(1 - (-t)²) is the same as √(1 - t²). Arctan is an odd function, but here the argument is even, so arctan(√(1 - t²)) is even. So the entire integrand is even. Therefore, we can write the integral as 2 times the integral from 0 to 1 of [1/(1 - t²)] arctan(√(1 - t²)) dt. That's helpful.

Now, let's focus on ∫₀¹ [1/(1 - t²)] arctan(√(1 - t²)) dt. Maybe another substitution. Let me set u = √(1 - t²). Then u² = 1 - t², so 2u du = -2t dt → t dt = -u du. Wait, but we have dt in terms of u. Let's see. If u = √(1 - t²), then t = √(1 - u²). Hmm, maybe not the best approach. Alternatively, let's try substitution for the arctan. Let’s set y = √(1 - t²). Then dy/dt = (1/(2√(1 - t²)))(-2t) = -t / √(1 - t²). Hmm, not sure. Alternatively, maybe integrate by parts. Let’s consider integrating [1/(1 - t²)] arctan(√(1 - t²)). Let me set u = arctan(√(1 - t²)), dv = dt/(1 - t²). Then du = derivative of arctan(y) where y = √(1 - t²). So du = [1/(1 + y²)] * (dy/dt) dt. y = √(1 - t²), so dy/dt = (1/(2√(1 - t²)))(-2t) = -t / √(1 - t²). Then du = [1/(1 + (1 - t²))] * (-t / √(1 - t²)) dt. The denominator 1 + y² = 1 + (1 - t²) = 2 - t². So du = [-t / ( (2 - t²) √(1 - t²) ) ] dt. And dv = dt/(1 - t²), so v = (1/2) ln |(1 + t)/(1 - t)|. So integration by parts gives uv - ∫ v du. Let's compute uv: arctan(√(1 - t²)) * (1/2) ln((1 + t)/(1 - t)) evaluated from 0 to 1, minus ∫₀¹ (1/2) ln((1 + t)/(1 - t)) * [-t / ( (2 - t²) √(1 - t²) ) ] dt. Hmm, this seems more complicated. Maybe not the best approach. Let me think again.

Alternatively, maybe a substitution to handle the arctan. Let’s set θ = arctan(√(1 - t²)). Then tanθ = √(1 - t²). Let’s square both sides: tan²θ = 1 - t² → t² = 1 - tan²θ. Then t = √(1 - tan²θ). Differentiating both sides: dt = [ (-2 tanθ sec²θ) / (2√(1 - tan²θ)) ) ] dθ. Wait, this might not be helpful. Alternatively, maybe set θ = √(1 - t²). Then θ = √(1 - t²) → θ² = 1 - t² → t = √(1 - θ²). Then dt = (-θ)/√(1 - θ²) dθ. Hmm, substituting into the integral. Let's see, when t=0, θ=1; t=1, θ=0. So the integral becomes from θ=1 to θ=0. The integrand is [1/(1 - t²)] arctan(θ) dt. But 1 - t² = θ², so 1/(1 - t²) = 1/θ². Then the integral becomes ∫₁⁰ [1/θ²] arctan(θ) * (-θ)/√(1 - θ²) dθ. The negative sign flips the limits: ∫₀¹ [1/θ²] arctan(θ) * (θ)/√(1 - θ²) dθ = ∫₀¹ [1/θ] arctan(θ) / √(1 - θ²) dθ. Hmm, not sure if that's better. Maybe another substitution here. Let’s set u = θ. Wait, not helpful. Alternatively, expand arctan(θ) as a power series. Maybe integrate term by term. Let me recall that arctan(z) = Σ_{n=0}^∞ (-1)^n z^{2n+1}/(2n+1) for |z| ≤1. Here θ is between 0 and 1, so that's valid. So arctan(θ) = Σ_{n=0}^∞ (-1)^n θ^{2n+1}/(2n+1). Then the integral becomes ∫₀¹ [1/θ] * Σ_{n=0}^∞ (-1)^n θ^{2n+1}/(2n+1) / √(1 - θ²) dθ = Σ_{n=0}^∞ (-1)^n/(2n+1) ∫₀¹ θ^{2n} / √(1 - θ²) dθ. Let’s compute the integral ∫₀¹ θ^{2n} / √(1 - θ²) dθ. Let’s substitute u = θ², then du = 2θ dθ, but maybe better to use substitution θ = sinφ. Let θ = sinφ, so when θ=0, φ=0; θ=1, φ=π/2. Then dθ = cosφ dφ. The integral becomes ∫₀^{π/2} (sinφ)^{2n} / √(1 - sin²φ) * cosφ dφ = ∫₀^{π/2} (sin^{2n}φ) / cosφ * cosφ dφ = ∫₀^{π/2} sin^{2n}φ dφ. That's a standard integral, which is (π/2) * ( (2n)! ) / (4^n (n!)^2 ) ). So the integral ∫₀¹ θ^{2n} / √(1 - θ²) dθ = (π/2) * ( (2n)! ) / (4^n (n!)^2 ). Therefore, the original sum becomes Σ_{n=0}^∞ (-1)^n/(2n+1) * (π/2) * ( (2n)! ) / (4^n (n!)^2 ). Hmm, this seems complicated, but maybe it can be simplified. Let me write it as (π/2) Σ_{n=0}^∞ [ (-1)^n (2n)! ] / [ (2n+1) 4^n (n!)^2 ) ].

Wait, the term (2n)! / (4^n (n!)^2) is the central binomial coefficient divided by 4^n. The central binomial coefficient is (2n choose n) = (2n)! / (n!)^2. So this term is (2n choose n) / 4^n. So the sum becomes (π/2) Σ_{n=0}^∞ [ (-1)^n (2n choose n) ] / [ (2n+1) 4^n ].

Hmm, I wonder if this sum has a closed form. Let me recall that generating functions for central binomial coefficients. For example, Σ_{n=0}^∞ (2n choose n) x^n = 1/√(1 - 4x) for |x| < 1/4. But here we have (-1)^n / 4^n, so x = -1/4. Then Σ_{n=0}^∞ (2n choose n) (-1/4)^n = 1/√(1 - 4*(-1/4)) = 1/√(1 +1) = 1/√2. But our sum is Σ [ (2n choose n) (-1/4)^n ] / (2n+1). Hmm, integrating the generating function? Let me think. Let’s consider that Σ_{n=0}^∞ (2n choose n) x^n = 1/√(1 - 4x). Then integrating term by term from 0 to x: ∫₀^x Σ_{n=0}^∞ (2n choose n) t^n dt = Σ_{n=0}^∞ (2n choose n) x^{n+1}/(n+1). But we have Σ_{n=0}^∞ (2n choose n) x^n / (2n+1). Let’s adjust indices. Let m = n + 1, but not sure. Alternatively, note that 1/(2n+1) = ∫₀^1 t^{2n} dt. So Σ_{n=0}^∞ (2n choose n) x^n / (2n+1) = Σ_{n=0}^∞ (2n choose n) x^n ∫₀^1 t^{2n} dt = ∫₀^1 Σ_{n=0}^∞ (2n choose n) (x t²)^n dt = ∫₀^1 1/√(1 - 4x t²) dt. So substituting x = -1/4, we get ∫₀^1 1/√(1 - 4*(-1/4) t²) dt = ∫₀^1 1/√(1 + t²) dt. The integral of 1/√(1 + t²) dt is sinh^{-1}(t) from 0 to1, which is ln(1 + √2). Therefore, Σ_{n=0}^∞ (2n choose n) (-1/4)^n / (2n+1) = ln(1 + √2). Therefore, our original sum is (π/2) * ln(1 + √2). Therefore, the integral from 0 to1 of [1/(1 - t²)] arctan(√(1 - t²)) dt = (π/2) * ln(1 + √2). Then the original integral was 2 times this, so the total integral is 2 * (π/2) * ln(1 + √2) = π ln(1 + √2).

Wait, let me verify this step again. The integral after substitution was ∫₀¹ [1/(1 - t²)] arctan(√(1 - t²)) dt = (π/2) * Σ_{n=0}^∞ [ (-1)^n (2n choose n) ] / [ (2n+1) 4^n ] = (π/2) * ln(1 + √2). Then multiplying by 2 gives π ln(1 + √2). That seems correct. Let me check the steps again. The substitution steps leading to the series expansion, then recognizing the integral as related to the generating function, and then integrating to get ln(1 + √2). Yes, that makes sense. So the exact answer is π times the natural logarithm of 1 plus square root of 2.

Now, let's compute the numerical approximation. ln(1 + √2) is approximately ln(2.41421356237). Let me calculate that. √2 ≈ 1.41421356237, so 1 + √2 ≈ 2.41421356237. The natural log of that: ln(2.41421356237) ≈ 0.88137358702. Then multiply by π (≈3.1415926535) gives approximately 0.88137358702 * 3.1415926535 ≈ 2.7686592831. Let me check with a calculator. 0.88137358702 * 3.1415926535: 0.8 * 3.14159 ≈ 2.51327, 0.08 *3.14159≈0.251327, 0.001373587*3.14159≈0.004315. Adding up: 2.51327 +0.251327=2.764597 +0.004315≈2.768912. So approximately 2.768912. Rounded to 10 decimal places, maybe 2.7689120014? Let me compute more accurately. Let's use more precise values. Let me compute ln(1 + √2):

√2 ≈ 1.4142135623730950488016887242097

1 + √2 ≈ 2.4142135623730950488016887242097

ln(2.4142135623730950488016887242097):

Using the Taylor series or calculator approximation. Let me recall that ln(2) ≈0.69314718056, ln(3)≈1.098612288668, so ln(2.4142) is between them. Alternatively, use the formula ln(1+√2) = arcsinh(1), since sinh(arcsinh(1))=1, and sinh(x) = (e^x - e^{-x})/2. Let me compute arcsinh(1). arcsinh(1) = ln(1 + √(1 +1)) = ln(1 + √2), which is exactly. So arcsinh(1) = ln(1 + √2). Therefore, ln(1 + √2) = arcsinh(1). The value of arcsinh(1) is approximately 0.88137358701954302523. Then multiplying by π (≈3.14159265358979323846) gives 0.88137358701954302523 * 3.14159265358979323846 ≈ 2.768659283312175599. Rounded to 10 decimal places: 2.7686592833.

So the numerical approximation is approximately 2.7686592833. Let me verify with another method. Alternatively, compute the integral numerically. Let's take x from 0 to 2, but the integrand has singularities at x=0 and x=2. However, the integral converges because near x=0, the integrand behaves like (1/x) arctan(√(2x)) ≈ (1/x) * √(2x) = √(2)/√x, which is integrable. Similarly near x=2. So the integral is convergent. But numerical integration might be tricky due to the singularities. But given that we have an analytical result, and the numerical approximation from that is about 2.7686592833, which seems reasonable.

Therefore, the exact answer is π ln(1 + √2), and the numerical approximation is approximately 2.7686592833.
</think>

{"answer": "\\pi \\ln(1 + \\sqrt{2})", "numerical_answer": 2.7686592833}