We will show that the integral

  I = ∫₀¹ K(√x) E(√(1–x)) dx

can be written in closed‐form. (Here K(k) and E(k) are the complete elliptic integrals of the first and second kinds defined by

  K(k) = ∫₀^(π/2) (1 – k² sin²θ)^(-1/2) dθ  and  E(k) = ∫₀^(π/2) (1 – k² sin²θ)^(1/2) dθ.)

One way to show the answer is to use the known series representations. In particular one may write

  K(√x) = (π/2) Σₘ₌₀^∞ [(1/2)₍ₘ₎/(m!)²] x^m     (1)
  E(√(1–x)) = (π/2) Σₙ₌₀^∞ [ (–1/2)₍ₙ₎/(n!)² ] (1–x)^n     (2)

where (a)₍ₘ₎ is the Pochhammer symbol. Then the product is

  K(√x)E(√(1–x)) = (π²/4) Σₘ₌₀^∞ Σₙ₌₀^∞ [(1/2)₍ₘ₎ (–1/2)₍ₙ₎/(m!)²(n!)²] x^m (1–x)^n.

Now, integrating term‐by‐term we use

  ∫₀¹ x^m (1–x)^n dx = B(m+1, n+1) = m! n!/ (m+n+1)!.

Thus
  I = (π²/4) Σₘ,ₙ≥0 [(1/2)₍ₘ₎ (–1/2)₍ₙ₎/(m! n!)] · 1/(m+n+1)!.    (3)

It is now convenient to write the double‐sum in “diagonal” form. Write k = m+n so that

  I = (π²/4) Σₖ₌₀^∞ 1/(k+1)! Σₘ₌₀ᵏ [(1/2)₍ₘ₎/(m!)] [ (–1/2)₍ₖ₋ₘ₎/((k–m)!) ].    (4)

But note that the two inner sums are nothing other than the Cauchy product of the series for
  Σₘ₌₀^∞ (1/2)₍ₘ₎/(m!) z^m = (1–z)^(-1/2)
and
  Σₙ₌₀^∞ (–1/2)₍ₙ₎/(n!) z^n = (1–z)^(1/2).
Their product is identically 1 so that when one equates coefficients one finds that for k ≥ 1 the inner sum is 0 and for k = 0 it is 1. (In other words, the convolution of the two sequences gives the coefficients in the expansion of 1 = 1 + 0·z + 0·z² + ⋯.)

Thus only the k = 0 term survives in (4) so that

  I = (π²/4) · 1/(0+1)! = π²/4.

A numerical evaluation gives

  π²/4 ≈ 2.4674011003.

In summary, the exact answer is

  I = π²/4.

The final answer in the required JSON format is shown below. 

{"answer": "\\frac{\\pi^2}{4}", "numerical_answer": "2.4674011003"}