Let's follow the steps:

1. **Find where the integrand changes sign**

We have \(|1+2\sin x|\).

Set \(1+2\sin x = 0\):

\[
2\sin x = -1 \implies \sin x = -\frac{1}{2}
\]

Within \(x \in [0, 2\pi]\), the solutions are:

\[
x_1 = \arcsin\left(-\frac{1}{2}\right) = \frac{7\pi}{6} \\
x_2 = 2\pi - \arcsin\left(-\frac{1}{2}\right) = \frac{11\pi}{6}
\]

So on \([0, 2\pi]\), \(1+2\sin x \geq 0\) for \(x \in [0,\frac{7\pi}{6}] \cup [\frac{11\pi}{6}, 2\pi]\), and negative in between.

**Let's check the sign in each region:**

- For \(x = 0\): \(\sin 0 = 0\), so \(1+2\times 0 = 1 > 0\)
- For \(x = \pi\): \(\sin \pi = 0\), so \(1+2\times 0 = 1 > 0\)
- For \(x = \frac{3\pi}{2}\): \(\sin \frac{3\pi}{2} = -1\), \(1 + 2\times (-1) = 1-2 = -1 < 0\)

Plug in values between points to confirm:

- On \([0, \frac{7\pi}{6}]\), it's positive.
- Between \(\frac{7\pi}{6}\) and \(\frac{11\pi}{6}\), it's negative.
- On \([\frac{11\pi}{6}, 2\pi]\), it's positive.

2. **Break up the integral at the critical points:**

\[
\int_0^{2\pi}\left|1+2\sin x\right|dx
= \int_0^{\frac{7\pi}{6}} (1 + 2\sin x) dx
+ \int_{\frac{7\pi}{6}}^{\frac{11\pi}{6}} -(1+2\sin x) dx
+ \int_{\frac{11\pi}{6}}^{2\pi} (1 + 2\sin x) dx
\]

3. **Compute each integral**

First, find the indefinite integral:

\[
\int (1 + 2\sin x) dx = x - 2\cos x + C
\]

So,

- \(I_1 = \int_0^{\frac{7\pi}{6}} (1 + 2\sin x) dx = [x - 2\cos x]_{0}^{\frac{7\pi}{6}}\)
- \(I_2 = -\int_{\frac{7\pi}{6}}^{\frac{11\pi}{6}} (1 + 2\sin x) dx = -\left([x - 2\cos x]_{\frac{7\pi}{6}}^{\frac{11\pi}{6}}\right)\)
- \(I_3 = \int_{\frac{11\pi}{6}}^{2\pi} (1 + 2\sin x) dx = [x - 2\cos x]_{\frac{11\pi}{6}}^{2\pi}\)

Now, sum up:

\[
\text{Total} = I_1 + I_2 + I_3
\]

Letâ€™s compute each:

#### \(I_1\):

\[
I_1 = \left[\frac{7\pi}{6} - 2\cos\left(\frac{7\pi}{6}\right)\right] - [0 - 2\cos 0]
\]

Recall:

- \(\cos(0) = 1\)
- \(\cos\left(\frac{7\pi}{6}\right) = \cos(\pi + \frac{\pi}{6}) = -\cos\left(\frac{\pi}{6}\right) = -\frac{\sqrt{3}}{2}\)

So,

\[
I_1 = \frac{7\pi}{6} - 2(-\frac{\sqrt{3}}{2}) - (0 - 2\times 1)
= \frac{7\pi}{6} + \sqrt{3} - (-2)
= \frac{7\pi}{6} + \sqrt{3} + 2
\]

#### \(I_2\):

\[
I_2 = -\left\{ \left[\frac{11\pi}{6} - 2\cos\left(\frac{11\pi}{6}\right)\right] - \left[\frac{7\pi}{6} - 2\cos\left(\frac{7\pi}{6}\right)\right] \right\}
\]

Recall:

- \(\cos\left(\frac{11\pi}{6}\right) = \cos(2\pi - \frac{\pi}{6}) = \cos(\frac{\pi}{6}) = \frac{\sqrt{3}}{2}\)

So,

\[
I_2 = -\left\{ \left(\frac{11\pi}{6} - 2\times \frac{\sqrt{3}}{2} \right) - \left(\frac{7\pi}{6} - 2\times (-\frac{\sqrt{3}}{2})\right) \right\}
\]
\[
= -\left\{ \left( \frac{11\pi}{6} - \sqrt{3}\right) - \left( \frac{7\pi}{6} + \sqrt{3} \right) \right\}
\]
\[
= - \left( \frac{11\pi}{6} - \sqrt{3} - \frac{7\pi}{6} - \sqrt{3} \right)
\]
\[
= - \left( \frac{11\pi}{6} - \frac{7\pi}{6} - 2\sqrt{3} \right )
\]
\[
= - \left (\frac{4\pi}{6} - 2\sqrt{3} \right )
\]
\[
= - \left (\frac{2\pi}{3} - 2\sqrt{3} \right )
= -\frac{2\pi}{3} + 2\sqrt{3}
\]

#### \(I_3\):

\[
I_3 = \left[2\pi - 2\cos(2\pi)\right] - \left[\frac{11\pi}{6} - 2\cos\left(\frac{11\pi}{6}\right)\right]
\]

Recall:

- \(\cos(2\pi) = 1\)

So,

\[
I_3 = (2\pi - 2\times 1) - (\frac{11\pi}{6} - 2 \times \frac{\sqrt{3}}{2})
= (2\pi - 2) - (\frac{11\pi}{6} - \sqrt{3})
= 2\pi - 2 - \frac{11\pi}{6} + \sqrt{3}
\]

\[
= \left(2\pi - \frac{11\pi}{6}\right) + (\sqrt{3} - 2)
= \left(\frac{12\pi}{6} - \frac{11\pi}{6}\right) + (\sqrt{3} - 2)
= \frac{\pi}{6} + (\sqrt{3} - 2)
= \frac{\pi}{6} + \sqrt{3} - 2
\]

4. **Add the terms:**

Sum \(I_1, I_2, I_3\):

\[
I_1: \frac{7\pi}{6} + \sqrt{3} + 2 \\
I_2: -\frac{2\pi}{3} + 2\sqrt{3} \\
I_3: \frac{\pi}{6} + \sqrt{3} - 2
\]

Sum:

\[
\left(\frac{7\pi}{6} + \sqrt{3} + 2\right) 
+ \left(-\frac{2\pi}{3} + 2\sqrt{3}\right)
+ \left(\frac{\pi}{6} + \sqrt{3} - 2\right)
\]

First, sum the \(\pi\) terms:

\[
\frac{7\pi}{6} - \frac{2\pi}{3} + \frac{\pi}{6}
\]

Write \(-\frac{2\pi}{3} = -\frac{4\pi}{6}\):

\[
\frac{7\pi}{6} - \frac{4\pi}{6} + \frac{\pi}{6} = \frac{(7 - 4 + 1)\pi}{6} = \frac{4\pi}{6} = \frac{2\pi}{3}
\]

Next, the \(\sqrt{3}\) terms:

\[
\sqrt{3} + 2\sqrt{3} + \sqrt{3} = (1 + 2 + 1)\sqrt{3} = 4\sqrt{3}
\]

Finally, the constants:

\[
2 + (-2) = 0
\]

So total is:

\[
\frac{2\pi}{3} + 4\sqrt{3}
\]

5. **Numerical approximation:**

\[
\frac{2\pi}{3} + 4\sqrt{3} \approx \frac{2 \times 3.1415926536}{3} + 4 \times 1.7320508076
\]
\[
= 2.0943951024 + 6.9282032304 = 9.0225983328
\]

Rounded to 10 decimal places:

\[
9.0225983328
\]

6. **JSON output:**

```json
{"answer": "\\frac{2\\pi}{3} + 4\\sqrt{3}", "numerical_answer": "9.0225983328"}
```