# Evaluating the Definite Integral

I'll evaluate the definite integral:
$$\int\limits_0^2 x^{(2 \cdot 1 - 1)/4}(2 - x)^{0.5/2}J_{1 - 0.5}(1 \cdot \sqrt{x})J_{0.5}(1 \cdot \sqrt{2 - x})\:dx$$

## Step 1: Simplify the expression

First, let's simplify the exponents:
- $(2 \cdot 1 - 1)/4 = 1/4$
- $0.5/2 = 1/4$
- $J_{1 - 0.5} = J_{0.5}$

So our integral becomes:
$$\int\limits_0^2 x^{1/4}(2 - x)^{1/4}J_{0.5}(\sqrt{x})J_{0.5}(\sqrt{2 - x})\:dx$$

## Step 2: Use the Weber-Schafheitlin integral formula

This integral can be evaluated using a specialized form of the Weber-Schafheitlin discontinuous integral. The formula we need is:

$$\int_0^a x^{\mu}(a-x)^{\nu}J_{\mu}(px)J_{\nu}(q\sqrt{a-x})dx = \frac{a^{\mu+\nu+1}}{2^{\nu}p^{\mu+1}q^{\nu}}J_{\mu+\nu+1}(\sqrt{a}p)$$

where $\text{Re}(\mu) > -1$, $\text{Re}(\nu) > -1$, and $p,q > 0$.

In our case:
- $a = 2$
- $\mu = 1/4$
- $\nu = 1/4$
- $p = 1$
- $q = 1$

## Step 3: Apply the formula to our integral

Substituting these values:

$$\int\limits_0^2 x^{1/4}(2 - x)^{1/4}J_{0.5}(\sqrt{x})J_{0.5}(\sqrt{2 - x})\:dx = \frac{2^{1/4+1/4+1}}{2^{1/4} \cdot 1^{1/4+1} \cdot 1^{1/4}}J_{1/4+1/4+1}(\sqrt{2} \cdot 1)$$

Simplifying:
$$= \frac{2^{1/2+1}}{2^{1/4} \cdot 1 \cdot 1}J_{1/2+1}(\sqrt{2})$$

$$= \frac{2^{3/2}}{2^{1/4}}J_{3/2}(\sqrt{2})$$

$$= 2^{5/4}J_{3/2}(\sqrt{2})$$

## Step 4: Evaluate $J_{3/2}(\sqrt{2})$

For Bessel functions of half-integer order, we have a closed form:

$$J_{n+1/2}(z) = \sqrt{\frac{2}{\pi z}} \left( \sin(z) P_n(\cos z) - \cos(z) Q_n(\cos z) \right)$$

where $P_n$ and $Q_n$ are polynomials.

For $J_{3/2}(z)$, the formula simplifies to:

$$J_{3/2}(z) = \sqrt{\frac{2}{\pi z}} \left( \frac{\sin z}{z} - \frac{\cos z}{z} \right)$$

So:

$$J_{3/2}(\sqrt{2}) = \sqrt{\frac{2}{\pi \sqrt{2}}} \left( \frac{\sin \sqrt{2}}{\sqrt{2}} - \frac{\cos \sqrt{2}}{\sqrt{2}} \right)$$

$$= \sqrt{\frac{2}{\pi \sqrt{2}}} \cdot \frac{1}{\sqrt{2}} \left( \sin \sqrt{2} - \cos \sqrt{2} \right)$$

$$= \sqrt{\frac{2}{\pi}} \cdot \frac{1}{2} \left( \sin \sqrt{2} - \cos \sqrt{2} \right)$$

$$= \frac{1}{\sqrt{2\pi}} \left( \sin \sqrt{2} - \cos \sqrt{2} \right)$$

## Step 5: Calculate the final result

Putting it all together:

$$\int\limits_0^2 x^{1/4}(2 - x)^{1/4}J_{0.5}(\sqrt{x})J_{0.5}(\sqrt{2 - x})\:dx = 2^{5/4} \cdot \frac{1}{\sqrt{2\pi}} \left( \sin \sqrt{2} - \cos \sqrt{2} \right)$$

$$= \frac{2^{5/4}}{\sqrt{2\pi}} \left( \sin \sqrt{2} - \cos \sqrt{2} \right)$$

$$= \frac{2^{5/4}}{\sqrt{2\pi}} \sin(\sqrt{2} - \pi/4)$$

## Step 6: Numerical approximation

Computing this value:
- $2^{5/4} \approx 2.3784142300$
- $\sqrt{2\pi} \approx 2.5066282746$
- $\sin \sqrt{2} \approx 0.9524129804$
- $\cos \sqrt{2} \approx 0.3048106211$
- $\sin \sqrt{2} - \cos \sqrt{2} \approx 0.6476023593$

Therefore:
$$\frac{2^{5/4}}{\sqrt{2\pi}} \left( \sin \sqrt{2} - \cos \sqrt{2} \right) \approx \frac{2.3784142300}{2.5066282746} \cdot 0.6476023593 \approx 0.6145030397$$

{"answer": "\\frac{2^{5/4}}{\\sqrt{2\\pi}}(\\sin\\sqrt{2} - \\cos\\sqrt{2})", "numerical_answer": "0.6145030397"}