# Evaluating the definite integral $\int_0^{\frac{1}{2}}\left\lfloor\frac{1}{x}\right\rfloor\left\lceil\frac{1}{x}\right\rceil\ln\left(1-\frac{1}{\left\lfloor\frac{1}{x}\right\rfloor^2}\right)\mathrm{d}x$

## Step 1: Analyze the floor and ceiling functions

Let's first understand how $\lfloor\frac{1}{x}\rfloor$ and $\lceil\frac{1}{x}\rceil$ behave in the interval $(0,\frac{1}{2}]$.

For $x \in (0,\frac{1}{2}]$, we have $\frac{1}{x} \geq 2$. More specifically:
- When $\frac{1}{n+1} < x \leq \frac{1}{n}$ where $n \geq 2$, we have:
  - $\lfloor\frac{1}{x}\rfloor = n$
  - $\lceil\frac{1}{x}\rceil = n+1$

## Step 2: Break down the integral into subintervals

We need to break the integral into subintervals where the floor and ceiling functions are constant:

$$\int_0^{\frac{1}{2}}\left\lfloor\frac{1}{x}\right\rfloor\left\lceil\frac{1}{x}\right\rceil\ln\left(1-\frac{1}{\left\lfloor\frac{1}{x}\right\rfloor^2}\right)\mathrm{d}x = \sum_{n=2}^{\infty}\int_{\frac{1}{n+1}}^{\frac{1}{n}}n(n+1)\ln\left(1-\frac{1}{n^2}\right)\mathrm{d}x$$

## Step 3: Simplify the expression in each subinterval

In each subinterval $[\frac{1}{n+1}, \frac{1}{n}]$, our integrand simplifies to:
$$n(n+1)\ln\left(1-\frac{1}{n^2}\right)$$

Let's compute the integral for each subinterval:
$$\int_{\frac{1}{n+1}}^{\frac{1}{n}}n(n+1)\ln\left(1-\frac{1}{n^2}\right)\mathrm{d}x = n(n+1)\ln\left(1-\frac{1}{n^2}\right)\left[\frac{1}{n} - \frac{1}{n+1}\right]$$

$$= n(n+1)\ln\left(1-\frac{1}{n^2}\right)\frac{1}{n(n+1)} = \ln\left(1-\frac{1}{n^2}\right)$$

## Step 4: Evaluate the infinite sum

The integral becomes:
$$\int_0^{\frac{1}{2}}\left\lfloor\frac{1}{x}\right\rfloor\left\lceil\frac{1}{x}\right\rceil\ln\left(1-\frac{1}{\left\lfloor\frac{1}{x}\right\rfloor^2}\right)\mathrm{d}x = \sum_{n=2}^{\infty}\ln\left(1-\frac{1}{n^2}\right)$$

Let's simplify this sum. Note that:
$$1-\frac{1}{n^2} = \frac{n^2-1}{n^2} = \frac{(n-1)(n+1)}{n^2}$$

So:
$$\ln\left(1-\frac{1}{n^2}\right) = \ln\left(\frac{(n-1)(n+1)}{n^2}\right) = \ln\left(\frac{n-1}{n}\right) + \ln\left(\frac{n+1}{n}\right)$$

This gives us:
$$\sum_{n=2}^{\infty}\ln\left(1-\frac{1}{n^2}\right) = \sum_{n=2}^{\infty}\left[\ln\left(\frac{n-1}{n}\right) + \ln\left(\frac{n+1}{n}\right)\right]$$

Let's look at these two terms separately:

For the first term:
$$\sum_{n=2}^{\infty}\ln\left(\frac{n-1}{n}\right) = \sum_{n=2}^{\infty}\ln\left(1-\frac{1}{n}\right) = \ln\left(\frac{1}{2}\right) + \ln\left(\frac{2}{3}\right) + \ln\left(\frac{3}{4}\right) + \cdots$$

For the second term:
$$\sum_{n=2}^{\infty}\ln\left(\frac{n+1}{n}\right) = \sum_{n=2}^{\infty}\ln\left(1+\frac{1}{n}\right) = \ln\left(\frac{3}{2}\right) + \ln\left(\frac{4}{3}\right) + \ln\left(\frac{5}{4}\right) + \cdots$$

These are telescoping series. Let's see what happens:
$$\sum_{n=2}^{\infty}\ln\left(\frac{n-1}{n}\right) = \lim_{m\to\infty}\sum_{n=2}^{m}\ln\left(\frac{n-1}{n}\right) = \lim_{m\to\infty}\ln\left(\frac{1}{m}\right) = -\infty$$

However, the combined sum is finite because:
$$\sum_{n=2}^{\infty}\left[\ln\left(\frac{n-1}{n}\right) + \ln\left(\frac{n+1}{n}\right)\right] = \lim_{m\to\infty}\ln\left(\frac{1 \cdot 3 \cdot 4 \cdot 6 \cdot \cdots \cdot (m-1) \cdot (m+1)}{2 \cdot 2 \cdot 3 \cdot 4 \cdot \cdots \cdot m \cdot m}\right)$$

This simplifies considerably through cancellation. When we write out the first few terms:
$$\ln\left(\frac{1}{2}\right) + \ln\left(\frac{3}{2}\right) + \ln\left(\frac{2}{3}\right) + \ln\left(\frac{4}{3}\right) + \ln\left(\frac{3}{4}\right) + \cdots$$

We notice a pattern where many terms cancel. For a finite upper limit $m$, the sum becomes:
$$\ln\left(\frac{1 \cdot (m+1)}{2 \cdot m}\right) = \ln\left(\frac{m+1}{2m}\right)$$

As $m \to \infty$, $\frac{m+1}{2m} \to \frac{1}{2}$, so:
$$\sum_{n=2}^{\infty}\ln\left(1-\frac{1}{n^2}\right) = \ln\left(\frac{1}{2}\right) = -\ln(2)$$

## Step 5: Final result

$$\int_0^{\frac{1}{2}}\left\lfloor\frac{1}{x}\right\rfloor\left\lceil\frac{1}{x}\right\rceil\ln\left(1-\frac{1}{\left\lfloor\frac{1}{x}\right\rfloor^2}\right)\mathrm{d}x = -\ln(2)$$

Numerical approximation (to 10 decimal places):
$-\ln(2) \approx -0.6931471806$

{"answer": "-\\ln(2)", "numerical_answer": "-0.6931471806"}