

To solve the definite integral \( \int_{0}^{2} x^{-1/2}(2 - x)^{-1/2} \ln\left( \sqrt{x(2 - x)} + \sqrt{1 + x(2 - x)} \right) \, dx \), we proceed with the following steps:

### Step 1: Simplify the Integrand and Substitute Variables
First, we simplify the argument of the logarithm. Let \( t = x/2 \), so \( x = 2t \) and \( dx = 2dt \). The limits of integration change from \( x = 0 \) to \( t = 0 \) and \( x = 2 \) to \( t = 1 \). Substituting these into the integral, we rewrite the integrand:
\[
x^{-1/2}(2 - x)^{-1/2} = (2t)^{-1/2}(2 - 2t)^{-1/2} = 2^{-1} t^{-1/2}(1 - t)^{-1/2}.
\]
Multiplying by \( dx = 2dt \), the factor \( 2 \cdot 2^{-1} = 1 \), so the integral becomes:
\[
\int_{0}^{1} t^{-1/2}(1 - t)^{-1/2} \ln\left( \sqrt{4t(1 - t)} + \sqrt{1 + 4t(1 - t)} \right) dt.
\]
Simplifying the square roots, \( \sqrt{4t(1 - t)} = 2\sqrt{t(1 - t)} \), so the logarithm term becomes \( \ln\left( 2\sqrt{t(1 - t)} + \sqrt{1 + 4t(1 - t)} \right) \).

### Step 2: Trigonometric Substitution
Next, use \( t = \sin^2\theta \), so \( dt = 2\sin\theta\cos\theta d\theta \), \( t^{-1/2} = \csc\theta \), \( (1 - t)^{-1/2} = \sec\theta \), and \( \sqrt{t(1 - t)} = \sin\theta\cos\theta \). The integral transforms to:
\[
\int_{0}^{\pi/2} \csc\theta \sec\theta \cdot \ln\left( 2\sin\theta\cos\theta + \sqrt{1 + 4\sin^2\theta\cos^2\theta} \right) \cdot 2\sin\theta\cos\theta d\theta.
\]
Simplifying, \( \csc\theta \sec\theta \cdot 2\sin\theta\cos\theta = 2 \), and \( 2\sin\theta\cos\theta = \sin(2\theta) \), so the integral reduces to:
\[
2 \int_{0}^{\pi/2} \ln\left( \sin(2\theta) + \sqrt{1 + \sin^2(2\theta)} \right) d\theta.
\]
Let \( \phi = 2\theta \), so \( d\theta = d\phi/2 \) and the limits become \( \phi = 0 \) to \( \phi = \pi \). The integral becomes:
\[
\int_{0}^{\pi} \ln\left( \sin\phi + \sqrt{1 + \sin^2\phi} \right) d\phi.
\]

### Step 3: Recognize the Integral as Catalan's Constant
The integrand \( \ln\left( \sin\phi + \sqrt{1 + \sin^2\phi} \right) \) is the inverse hyperbolic sine function \( \sinh^{-1}(\sin\phi) \). Expanding \( \sinh^{-1}(\sin\phi) \) as a power series and integrating term-by-term over \( [0, \pi] \) shows the integral equals \( 2G \), where \( G \) is Catalan's constant (\( G \approx 0.915965594177 \)).

### Step 4: Numerical Approximation
Catalan's constant \( G \approx 0.915965594177 \), so \( 2G \approx 1.831931188354 \).

### Final Answer
The exact answer is \( 2G \) (where \( G \) is Catalan's constant), and the numerical approximation is approximately \( 1.8319311884 \).

```json
{"answer": "2G", "numerical_answer": "1.8319311884"}
```