To compute the definite integral \(\int_0^{\frac{\pi}{2}} x \ln(\sin x) \, dx\), we will follow these steps:

### Step 1: Use Symmetry and Known Results
First, recall the following known integral:
\[
\int_0^{\frac{\pi}{2}} \ln(\sin x) \, dx = -\frac{\pi}{2} \ln 2.
\]
This result can be derived using symmetry and properties of logarithmic integrals.

### Step 2: Introduce a Parameter
Consider the integral:
\[
I(a) = \int_0^{\frac{\pi}{2}} \sin^a x \, dx = \frac{\sqrt{\pi} \, \Gamma\left(\frac{a+1}{2}\right)}{2 \, \Gamma\left(\frac{a}{2} + 1\right)},
\]
where \(\Gamma\) is the gamma function. Differentiating \(I(a)\) with respect to \(a\) gives:
\[
I'(a) = \int_0^{\frac{\pi}{2}} \sin^a x \ln(\sin x) \, dx.
\]
Evaluating \(I'(0)\) will give us \(\int_0^{\frac{\pi}{2}} \ln(\sin x) \, dx\), which we already know. However, we need to find \(\int_0^{\frac{\pi}{2}} x \ln(\sin x) \, dx\).

### Step 3: Use Integration by Parts
Let \(u = x\) and \(dv = \ln(\sin x) \, dx\). Then \(du = dx\) and \(v\) is an antiderivative of \(\ln(\sin x)\). However, finding \(v\) explicitly is challenging, so we proceed differently.

### Step 4: Utilize Series Expansion
Express \(\ln(\sin x)\) as a series:
\[
\ln(\sin x) = \ln x + \sum_{k=1}^\infty \frac{(-1)^k B_{2k} (2x)^{2k}}{2k (2k)!}, \quad 0 < x < \pi,
\]
where \(B_{2k}\) are Bernoulli numbers. However, integrating term by term is complex.

### Step 5: Use Fourier Series
The Fourier series of \(\ln(2 \sin x)\) is:
\[
\ln(2 \sin x) = -\sum_{k=1}^\infty \frac{\cos(2k x)}{k}, \quad 0 < x < \pi.
\]
Thus,
\[
\ln(\sin x) = -\ln 2 - \sum_{k=1}^\infty \frac{\cos(2k x)}{k}.
\]
Substitute this into the integral:
\[
\int_0^{\frac{\pi}{2}} x \ln(\sin x) \, dx = -\ln 2 \int_0^{\frac{\pi}{2}} x \, dx - \sum_{k=1}^\infty \frac{1}{k} \int_0^{\frac{\pi}{2}} x \cos(2k x) \, dx.
\]
The first integral is straightforward:
\[
\int_0^{\frac{\pi}{2}} x \, dx = \frac{\pi^2}{8}.
\]
For the second integral, integrate by parts:
\[
\int x \cos(2k x) \, dx = \frac{x \sin(2k x)}{2k} + \frac{\cos(2k x)}{4k^2} + C.
\]
Evaluating from \(0\) to \(\frac{\pi}{2}}\):
\[
\left. \frac{x \sin(2k x)}{2k} \right|_0^{\frac{\pi}{2}} = \frac{\pi \sin(k \pi)}{4k} = 0 \quad \text{(since } \sin(k \pi) = 0\text{)},
\]
\[
\left. \frac{\cos(2k x)}{4k^2} \right|_0^{\frac{\pi}{2}} = \frac{\cos(k \pi) - 1}{4k^2} = \frac{(-1)^k - 1}{4k^2}.
\]
Thus,
\[
\int_0^{\frac{\pi}{2}} x \cos(2k x) \, dx = \frac{(-1)^k - 1}{4k^2}.
\]
Now, the sum becomes:
\[
\sum_{k=1}^\infty \frac{1}{k} \cdot \frac{(-1)^k - 1}{4k^2} = \frac{1}{4} \sum_{k=1}^\infty \frac{(-1)^k - 1}{k^3}.
\]
Separate the sum:
\[
\sum_{k=1}^\infty \frac{(-1)^k}{k^3} = -\eta(3) = -\frac{3}{4} \zeta(3),
\]
\[
\sum_{k=1}^\infty \frac{-1}{k^3} = -\zeta(3),
\]
where \(\eta(s)\) is the Dirichlet eta function and \(\zeta(s)\) is the Riemann zeta function. Thus,
\[
\frac{1}{4} \left( -\frac{3}{4} \zeta(3) - \zeta(3) \right) = \frac{1}{4} \left( -\frac{7}{4} \zeta(3) \right) = -\frac{7}{16} \zeta(3).
\]

### Step 6: Combine Results
Putting it all together:
\[
\int_0^{\frac{\pi}{2}} x \ln(\sin x) \, dx = -\ln 2 \cdot \frac{\pi^2}{8} - \left( -\frac{7}{16} \zeta(3) \right) = -\frac{\pi^2}{8} \ln 2 + \frac{7}{16} \zeta(3).
\]

### Step 7: Numerical Approximation
Using \(\zeta(3) \approx 1.2020569032\) and \(\pi \approx 3.1415926536\):
\[
-\frac{\pi^2}{8} \ln 2 + \frac{7}{16} \zeta(3) \approx -0.3084251375 + 0.5258998951 = 0.2174747576.
\]

### Final Answer
\[
\boxed{
{"answer": "-\frac{\pi^2}{8} \ln 2 + \frac{7}{16} \zeta(3)", "numerical_answer": "0.2174747576"}
}
\]