# Evaluating $\int_0^\infty\frac{\{x\}^{\lceil x\rceil}}{1+\lceil x\rceil}\text{ dx}$

I'll start by understanding the notation:
- $\lceil x \rceil$ represents the ceiling function (smallest integer greater than or equal to x)
- $\{x\}$ represents the fractional part of x, where $\{x\} = x - \lfloor x \rfloor$

## Step 1: Decompose the integral

Let's break the integral into intervals where $\lceil x \rceil$ is constant:

$$\int_0^\infty\frac{\{x\}^{\lceil x\rceil}}{1+\lceil x\rceil}\text{ dx} = \sum_{n=0}^{\infty}\int_{n}^{n+1}\frac{\{x\}^{n+1}}{1+(n+1)}\text{ dx}$$

For $x \in [n, n+1)$, we have $\lceil x \rceil = n+1$ and $\{x\} = x - n$.

## Step 2: Simplify the sum

$$\sum_{n=0}^{\infty}\int_{n}^{n+1}\frac{(x-n)^{n+1}}{n+2}\text{ dx}$$

Let's make a substitution $t = x - n$, so when $x = n$, $t = 0$, and when $x = n+1$, $t = 1$:

$$\sum_{n=0}^{\infty}\frac{1}{n+2}\int_{0}^{1}t^{n+1}\text{ dt}$$

## Step 3: Evaluate the inner integral

$$\int_{0}^{1}t^{n+1}\text{ dt} = \left[\frac{t^{n+2}}{n+2}\right]_{0}^{1} = \frac{1}{n+2}$$

## Step 4: Simplify the sum further

$$\sum_{n=0}^{\infty}\frac{1}{n+2} \cdot \frac{1}{n+2} = \sum_{n=0}^{\infty}\frac{1}{(n+2)^2}$$

Let $m = n+2$, so $n = m-2$. When $n = 0$, $m = 2$, and as $n \to \infty$, $m \to \infty$:

$$\sum_{m=2}^{\infty}\frac{1}{m^2} = \sum_{m=1}^{\infty}\frac{1}{m^2} - \frac{1}{1^2} = \zeta(2) - 1 = \frac{\pi^2}{6} - 1$$

## Step 5: Final result

$$\int_0^\infty\frac{\{x\}^{\lceil x\rceil}}{1+\lceil x\rceil}\text{ dx} = \frac{\pi^2}{6} - 1$$

## Step 6: Numerical approximation

$\frac{\pi^2}{6} - 1 \approx \frac{9.8696044011}{6} - 1 \approx 1.6449340668 - 1 \approx 0.6449340668$

Rounded to 10 decimal places: $0.6449340668$

{"answer": "\\frac{\\pi^2}{6} - 1", "numerical_answer": "0.6449340668"}