Let's denote the integral as:
\[
I = \int_{1}^{\pi/3} \sec(x)\left(\tan(x)\log(x) + \frac{1}{x}\right) dx
\]

Let's split the integral into two parts:
\[
I = \int_{1}^{\pi/3} \sec(x) \tan(x)\log(x) \, dx + \int_{1}^{\pi/3} \frac{\sec(x)}{x} dx
\]

#### Part 1: \( I_1 = \int_{1}^{\pi/3} \sec(x)\tan(x)\log(x) \, dx \)

Let us use integration by parts:

Let
- \( u = \log(x) \implies du = \frac{1}{x} dx \)
- \( dv = \sec(x) \tan(x) dx \implies v = \sec(x) \)

So,
\[
I_1 = u v \Big|_{1}^{\pi/3} - \int_{1}^{\pi/3} v \, du = \log(x)\sec(x) \Big|_{1}^{\pi/3} - \int_{1}^{\pi/3} \sec(x) \frac{1}{x} dx
\]
But notice that the second term is exactly the second integral, \( I_2 = \int_{1}^{\pi/3} \frac{\sec(x)}{x} dx \).

So,
\[
I_1 = \log(x)\sec(x) \Big|_{1}^{\pi/3} - I_2
\]

#### The original integral:

\[
I = I_1 + I_2 = [\log(x)\sec(x) \Big|_{1}^{\pi/3} - I_2] + I_2 = \log(x)\sec(x) \Big|_{1}^{\pi/3}
\]

Thus, the definite integral simplifies to:

\[
I = \log\left(\frac{\pi}{3}\right)\sec\left(\frac{\pi}{3}\right) - \log(1)\sec(1)
\]

We know \(\log(1) = 0\), so the second term vanishes.

Also, \(\sec\left(\frac{\pi}{3}\right) = \frac{1}{\cos\left(\frac{\pi}{3}\right)} = 2\).

So,
\[
I = \log\left(\frac{\pi}{3}\right) \cdot 2 = 2 \log\left(\frac{\pi}{3}\right)
\]

---

### Numerical Approximation

First, 
\[
\frac{\pi}{3} \approx 1.0471975512
\]
Now
\[
\log\left(\frac{\pi}{3}\right) \approx \log(1.0471975512) \approx 0.0460843892
\]
So,
\[
I \approx 2 \times 0.0460843892 = 0.0921687784
\]

---

```json
{"answer": "2 \\log\\left( \\frac{\\pi}{3} \\right)", "numerical_answer": "0.0921687784"}
```