# Evaluating the definite integral $\int_0^6 x+(x-3)^7+\sin(x-3)dx$

I'll split this into three parts and evaluate each separately:
- $\int_0^6 x dx$
- $\int_0^6 (x-3)^7 dx$
- $\int_0^6 \sin(x-3) dx$

## Part 1: $\int_0^6 x dx$

The antiderivative of $x$ is $\frac{x^2}{2}$, so:
$\int_0^6 x dx = \left[\frac{x^2}{2}\right]_0^6 = \frac{6^2}{2} - \frac{0^2}{2} = \frac{36}{2} = 18$

## Part 2: $\int_0^6 (x-3)^7 dx$

Let's use substitution. Let $u = x-3$, then $du = dx$.
When $x = 0$, $u = -3$
When $x = 6$, $u = 3$

So the integral becomes:
$\int_{-3}^{3} u^7 du = \left[\frac{u^8}{8}\right]_{-3}^{3} = \frac{3^8}{8} - \frac{(-3)^8}{8} = \frac{6561}{8} - \frac{6561}{8} = 0$

Note: $(-3)^8 = 3^8 = 6561$ because $(-3)^8$ has an even power.

## Part 3: $\int_0^6 \sin(x-3) dx$

Let's use substitution again. Let $v = x-3$, then $dv = dx$.
When $x = 0$, $v = -3$
When $x = 6$, $v = 3$

So the integral becomes:
$\int_{-3}^{3} \sin(v) dv = \left[-\cos(v)\right]_{-3}^{3} = -\cos(3) - (-\cos(-3)) = -\cos(3) + \cos(3) = 0$

Since $\cos$ is an even function, $\cos(-3) = \cos(3)$.

## Combining all parts

$\int_0^6 x+(x-3)^7+\sin(x-3)dx = 18 + 0 + 0 = 18$

## Numerical approximation

The exact value is 18, which as a decimal rounded to 10 places is 18.0000000000.

{"answer": "18", "numerical_answer": "18.0000000000"}