


To solve the definite integral \(\int\limits_{0}^{\infty}\frac{x^{3}}{e^x-1}\left[8\cosh\left(0.5x\right)-\cosh\left(0.25x\right)\right]dx\), we proceed as follows:

### Step 1: Expand the hyperbolic cosine terms
Using the identity \(\cosh(z) = \frac{e^z + e^{-z}}{2}\), we rewrite the integrand:
\[
8\cosh(0.5x) - \cosh(0.25x) = 4\left(e^{0.5x} + e^{-0.5x}\right) - \frac{1}{2}\left(e^{0.25x} + e^{-0.25x}\right).
\]
Thus, the integral becomes:
\[
\int_{0}^{\infty} \frac{x^3}{e^x - 1} \left[4\left(e^{0.5x} + e^{-0.5x}\right) - \frac{1}{2}\left(e^{0.25x} + e^{-0.25x}\right)\right] dx.
\]

### Step 2: Split the integral into four terms
We split the integral into four separate integrals:
\[
4\int_{0}^{\infty} \frac{x^3 e^{0.5x}}{e^x - 1} dx + 4\int_{0}^{\infty} \frac{x^3 e^{-0.5x}}{e^x - 1} dx - \frac{1}{2}\int_{0}^{\infty} \frac{x^3 e^{0.25x}}{e^x - 1} dx - \frac{1}{2}\int_{0}^{\infty} \frac{x^3 e^{-0.25x}}{e^x - 1} dx.
\]

### Step 3: Use the series expansion of \(\frac{1}{e^x - 1}\)
For \(x > 0\), \(\frac{1}{e^x - 1} = \sum_{n=1}^{\infty} e^{-nx}\). Substituting this into each term, we rewrite the integrals as sums:
\[
4\sum_{n=1}^{\infty} \int_{0}^{\infty} x^3 e^{-(n - 0.5)x} dx + 4\sum_{n=1}^{\infty} \int_{0}^{\infty} x^3 e^{-(n + 0.5)x} dx - \frac{1}{2}\sum_{n=1}^{\infty} \int_{0}^{\infty} x^3 e^{-(n - 0.25)x} dx - \frac{1}{2}\sum_{n=1}^{\infty} \int_{0}^{\infty} x^3 e^{-(n + 0.25)x} dx.
\]

### Step 4: Evaluate the Gaussian integrals
The integral \(\int_{0}^{\infty} x^3 e^{-kx} dx = \frac{6}{k^4}\) (since \(\Gamma(4) = 6\)). Substituting this, the integrals become:
\[
24\sum_{n=1}^{\infty} \frac{1}{(n - 0.5)^4} + 24\sum_{n=1}^{\infty} \frac{1}{(n + 0.5)^4} - 3\sum_{n=1}^{\infty} \frac{1}{(n - 0.25)^4} - 3\sum_{n=1}^{\infty} \frac{1}{(n + 0.25)^4}.
\]

### Step 5: Simplify the sums using Hurwitz zeta functions
Using properties of the Hurwitz zeta function \(\zeta(s, a) = \sum_{n=0}^{\infty} \frac{1}{(n + a)^s}\), we relate the sums to \(\zeta(4, a)\). Key cancellations occur:
- For \(a = 0.5\), the sums \(\sum_{n=1}^{\infty} \frac{1}{(n - 0.5)^4} + \sum_{n=1}^{\infty} \frac{1}{(n + 0.5)^4}\) simplify to \(30\zeta(4) - 16\).
- For \(a = 0.25\), the sums \(\sum_{n=1}^{\infty} \frac{1}{(n - 0.25)^4} + \sum_{n=1}^{\infty} \frac{1}{(n + 0.25)^4}\) simplify to \(240\zeta(4) - 256\).

### Step 6: Combine terms and cancel \(\zeta(4)\)
Substituting these results, the \(\zeta(4)\) terms cancel, leaving:
\[
24(30\zeta(4) - 16) - 3(240\zeta(4) - 256) = 384.
\]

### Numerical Approximation
The exact result is \(384\), so the numerical approximation is \(384.0000000000\).

{"answer": "384", "numerical_answer": "384.0000000000"}