

To solve the definite integral \(\int_1^2 \frac{9x + 4}{x^5 + 3x^2 + x} \, dx\), we proceed as follows:

### Step 1: Factor the Denominator
The denominator \(x^5 + 3x^2 + x\) can be factored by first extracting \(x\):
\[
x^5 + 3x^2 + x = x(x^4 + 3x + 1)
\]

### Step 2: Partial Fraction Decomposition
We decompose the integrand \(\frac{9x + 4}{x(x^4 + 3x + 1)}\) into partial fractions. Assume:
\[
\frac{9x + 4}{x(x^4 + 3x + 1)} = \frac{A}{x} + \frac{Bx^3 + Cx^2 + Dx + E}{x^4 + 3x + 1}
\]
Multiplying both sides by \(x(x^4 + 3x + 1)\) and equating coefficients, we find \(A = 4\), \(B = -4\), \(C = 0\), \(D = 0\), and \(E = -3\). Thus:
\[
\frac{9x + 4}{x(x^4 + 3x + 1)} = \frac{4}{x} - \frac{4x^3 + 3}{x^4 + 3x + 1}
\]

### Step 3: Integrate Term by Term
The first term integrates to \(4 \ln|x|\). For the second term, notice that the numerator \(4x^3 + 3\) is the derivative of the denominator \(x^4 + 3x + 1\). Thus:
\[
\int \frac{4x^3 + 3}{x^4 + 3x + 1} \, dx = \ln|x^4 + 3x + 1| + C
\]
Combining these results, the antiderivative is:
\[
F(x) = 4 \ln x - \ln(x^4 + 3x + 1) + C
\]

### Step 4: Evaluate the Definite Integral
Evaluate \(F(x)\) from \(1\) to \(2\):
\[
F(2) - F(1) = \left[4 \ln 2 - \ln(2^4 + 3 \cdot 2 + 1)\right] - \left[4 \ln 1 - \ln(1^4 + 3 \cdot 1 + 1)\right]
\]
Simplifying the arguments of the logarithms:
- At \(x = 2\): \(2^4 + 3 \cdot 2 + 1 = 16 + 6 + 1 = 23\)
- At \(x = 1\): \(1^4 + 3 \cdot 1 + 1 = 1 + 3 + 1 = 5\)
- Since \(\ln 1 = 0\), we get:
\[
F(2) - F(1) = 4 \ln 2 - \ln 23 + \ln 5 = \ln\left(\frac{2^4 \cdot 5}{23}\right) = \ln\left(\frac{80}{23}\right)
\]

### Step 5: Numerical Approximation
The numerical value of \(\ln\left(\frac{80}{23}\right)\) is approximately \(1.2469260703\) (rounded to 10 decimal places).

{"answer": "\(\ln\left(\frac{80}{23}\right)\)", "numerical_answer": "1.2469260703"}