Let's follow the steps as requested.

### **Step 1: Compute the integral analytically**

We are given:
\[
I = \int_{0}^{1} x^{-1/2}(1-x)^{-1/2} T_4\left(\sqrt{x(1-x)}\right) dx,
\]
where \( T_4(y) \) is the Chebyshev polynomial of degree 4.

**Chebyshev polynomial of degree 4:**
\[
T_4(y) = 8y^4 - 8y^2 + 1
\]

Let's substitute this into the integral:

\[
I = \int_{0}^{1} x^{-1/2}(1-x)^{-1/2} \left[ 8(\sqrt{x(1-x)})^4 - 8(\sqrt{x(1-x)})^2 + 1 \right] dx
\]
\[
= \int_{0}^{1} x^{-1/2}(1-x)^{-1/2} \left[ 8 (x(1-x))^2 - 8 x(1-x) + 1 \right] dx
\]
\[
= 8 \int_{0}^{1} x^{-1/2}(1-x)^{-1/2} (x(1-x))^2 dx - 8 \int_{0}^{1} x^{-1/2}(1-x)^{-1/2} x(1-x) dx + \int_{0}^{1} x^{-1/2}(1-x)^{-1/2} dx
\]

Let us denote:

\[
I = 8 I_1 - 8 I_2 + I_3
\]

Where:
- \( I_1 = \int_{0}^{1} x^{-1/2}(1-x)^{-1/2} (x(1-x))^2 dx \)
- \( I_2 = \int_{0}^{1} x^{-1/2}(1-x)^{-1/2} x(1-x) dx \)
- \( I_3 = \int_{0}^{1} x^{-1/2}(1-x)^{-1/2} dx \)

---

#### **Compute \( I_3 \):**

\[
I_3 = \int_{0}^{1} x^{-1/2}(1-x)^{-1/2} dx
\]
This is a Beta function \( B(a,b) = \int_{0}^{1} x^{a-1}(1-x)^{b-1} dx \), with \( a = b = 1/2 \):
\[
I_3 = B(1/2,1/2) = \frac{\Gamma(1/2)\Gamma(1/2)}{\Gamma(1)} = \frac{(\sqrt{\pi})^2}{1} = \pi
\]

---

#### **Compute \( I_2 \):**

\[
I_2 = \int_{0}^{1} x^{-1/2} (1-x)^{-1/2} x (1-x) dx
\]
\[
= \int_{0}^{1} x^{1-1/2} (1-x)^{1-1/2} dx = \int_{0}^{1} x^{1/2}(1-x)^{1/2} dx
\]

In general:
\[
\int_{0}^{1} x^{p-1}(1-x)^{q-1} dx = B(p,q) = \frac{\Gamma(p)\Gamma(q)}{\Gamma(p+q)}
\]
Here, \( p = q = 3/2 \):

\[
I_2 = B(3/2, 3/2) = \frac{\Gamma(3/2)^2}{\Gamma(3)}
\]

Recall:
- \(\Gamma(3/2) = \frac{1}{2}\sqrt{\pi}\)
- \(\Gamma(3) = 2!\ = 2\)

\[
I_2 = \frac{\left( \frac{1}{2} \sqrt{\pi} \right)^2}{2} = \frac{\frac{1}{4}\pi}{2} = \frac{\pi}{8}
\]

---

#### **Compute \( I_1 \):**

\[
I_1 = \int_{0}^{1} x^{-1/2}(1-x)^{-1/2}(x(1-x))^2 dx
= \int_{0}^{1} x^{-1/2}(1-x)^{-1/2} x^2 (1-x)^2 dx \\
= \int_{0}^{1} x^{2-1/2} (1-x)^{2-1/2} dx
= \int_{0}^{1} x^{3/2}(1-x)^{3/2} dx
\]

So \( p = q = 5/2 \):

\[
I_1 = B(5/2, 5/2) = \frac{\Gamma(5/2)^2}{\Gamma(5)}
\]

Recall:
- \(\Gamma(5/2) = \frac{3}{2} \cdot \frac{1}{2}\sqrt{\pi} = \frac{3}{4}\sqrt{\pi}\)
- \(\Gamma(5) = 4! = 24\)

\[
I_1 = \frac{ \left( \frac{3}{4}\sqrt{\pi} \right)^2 }{24 }
= \frac{9}{16} \pi \cdot \frac{1}{24}
= \frac{9\pi}{384}
\]

---

### **Step 2: Assemble the result**

Recall:
\[
I = 8 I_1 - 8 I_2 + I_3
\]

Substitute the answers:
- \(I_1 = \dfrac{9\pi}{384}\)
- \(I_2 = \dfrac{\pi}{8}\)
- \(I_3 = \pi\)

So:
\[
I = 8 \times \frac{9\pi}{384} - 8 \times \frac{\pi}{8} + \pi
= \frac{72\pi}{384} - \pi + \pi
= \frac{72\pi}{384}
\]
But let's check the \(-8 I_2 + I_3\) more carefully:

\[
8 I_1 - 8 I_2 + I_3 = 8 \frac{9\pi}{384} - 8 \frac{\pi}{8} + \pi
= \frac{72\pi}{384} - \pi + \pi
= \frac{72\pi}{384}
\]

Now, simplify \( \frac{72\pi}{384} \):

\[
\frac{72}{384} = \frac{72 \div 24}{384 \div 24} = \frac{3}{16}
\]

\[
I = \frac{3\pi}{16}
\]

---

### **Step 3: Numerical value**

\[
I = \frac{3\pi}{16}
\]

Letâ€™s compute this numerically:

\[
\pi \approx 3.1415926536
\]

\[
\frac{3 \cdot 3.1415926536}{16} = \frac{9.4247779608}{16} \approx 0.5890486226
\]

---

### **Step 4: Output the result as requested**

```json
{"answer": "\\frac{3\\pi}{16}", "numerical_answer": "0.5890486226"}
```