We wish to evaluate

  I = ∫₀² x · arctan(√(x(2 − x))) dx.

A useful trick is to make a substitution that exploits the symmetry in the integrand. First, set

  x = 1 + y   so that dx = dy,

which changes the limits from x = 0, 2 to y = −1, +1. Notice that

  2 − x = 2 − (1 + y) = 1 − y
  x(2 − x) = (1 + y)(1 − y) = 1 − y²,
  √(x(2 − x)) = √(1 − y²).

Then the integral becomes

  I = ∫₋₁¹ (1 + y) · arctan(√(1 − y²)) dy.

Now split the integral into two pieces:

  I = ∫₋₁¹ arctan(√(1 − y²)) dy + ∫₋₁¹ y · arctan(√(1 − y²)) dy.

The second integrand is an odd function (since y is odd and arctan(√(1 − y²)) is even) so its integral over [–1, 1] vanishes. Hence

  I = ∫₋₁¹ arctan(√(1 − y²)) dy
    = 2 ∫₀¹ arctan(√(1 − y²)) dy.   (1)

Now perform the substitution

  y = sinθ   with  dy = cosθ dθ,
  when y = 0, θ = 0 and when y = 1, θ = π/2.
Also, √(1 – y²) = √(1 – sin²θ) = cosθ (since cosθ ≥ 0 for θ in [0, π/2]). Hence (1) becomes

  I = 2 ∫₀^(π/2) arctan(cosθ) · cosθ dθ.   (2)

At this point it is natural to apply integration by parts. In (2) set

  u = arctan(cosθ)   ⇒ du = −(sinθ)/(1 + cos²θ) dθ,
  dv = cosθ dθ     ⇒ v = sinθ.

Then integration by parts yields

  I = 2 { [sinθ · arctan(cosθ)]₀^(π/2) − ∫₀^(π/2) sinθ · (−sinθ/(1 + cos²θ)) dθ }.
The boundary term is computed as follows:
  at θ = π/2, sin(π/2) = 1 and cos(π/2) = 0 so arctan(0) = 0;
  at θ = 0, sin0 = 0.
Thus the boundary term vanishes and

  I = 2 ∫₀^(π/2) (sin²θ/(1 + cos²θ)) dθ.   (3)

Now use the Pythagorean identity sin²θ = 1 − cos²θ so that

  I = 2 ∫₀^(π/2) [ (1 − cos²θ)/(1 + cos²θ) ] dθ
    = 2 [ ∫₀^(π/2) 1 dθ − ∫₀^(π/2) (2 cos²θ/(1 + cos²θ)) dθ ].
However, it is more convenient to split the fraction in another way. Write

  cos²θ/(1 + cos²θ) = 1 − 1/(1 + cos²θ),
so that
  (1 − cos²θ)/(1 + cos²θ) = 1 − [cos²θ/(1 + cos²θ)] = 1 − [1 − 1/(1 + cos²θ)] = 1/(1 + cos²θ).

Thus (3) becomes

  I = 2 ∫₀^(π/2) (1/(1 + cos²θ)) dθ.   (4)

We now need to evaluate

  K = ∫₀^(π/2) 1/(1 + cos²θ) dθ.

A standard method is to use the tangent substitution. Let

  t = tanθ  ⇒  θ = arctan t  and  dθ = dt/(1 + t²).

Since cosθ = 1/√(1+t²), we have cos²θ = 1/(1+t²), so that

  1 + cos²θ = 1 + 1/(1+t²) = (t² + 2)/(1+t²).

Thus the differential transforms as

  K = ∫_{t=0}^{∞} [1/((t²+2)/(1+t²))] · [dt/(1+t²)] = ∫₀^(∞) (1+t²)/(t²+2) · dt/(1+t²)
    = ∫₀^(∞) dt/(t²+2).

That is a standard integral. (Recall that ∫₀^(∞) dt/(t²+a²) = π/(2a).) Here a² = 2 so that a = √2. Hence

  K = π/(2√2).

Returning to (4), we have

  I = 2K = 2 · (π/(2√2)) = π/√2.   (5)

But wait! We must go back to check the steps. Notice that in an earlier step we had
  I = 2 ∫₀^(π/2) [sin²θ/(1 + cos²θ)] dθ.
Then writing cos²θ/(1+cos²θ) = 1 − 1/(1+cos²θ) we get
  sin²θ/(1+cos²θ) = [1 − cos²θ]/(1+cos²θ) = 1/(1+cos²θ) - ?
Let’s rework that step carefully:

We have 
  sin²θ = 1 − cos²θ.
So, 
  sin²θ/(1+cos²θ) = (1 − cos²θ)/(1+cos²θ) 
    = [ (1+cos²θ) − 2 cos²θ ]/(1+cos²θ)
    = 1 − (2 cos²θ)/(1+cos²θ).

Thus (3) becomes

  I = 2 [ ∫₀^(π/2) 1 dθ − 2∫₀^(π/2) (cos²θ/(1+cos²θ)) dθ ].
Now, note that
  cos²θ/(1+cos²θ) = 1 − 1/(1+cos²θ).
So that
  ∫₀^(π/2) cos²θ/(1+cos²θ) dθ = ∫₀^(π/2) 1 dθ − ∫₀^(π/2) 1/(1+cos²θ)dθ = (π/2) − K.
Thus we have

  I = 2 [ (π/2) − 2 ( (π/2) − K ) ] = 2 [ (π/2) − π + 2K ] = 2 [ −π/2 + 2K ] = −π + 4K.
Now substitute K = π/(2√2):

  I = −π + 4 (π/(2√2)) = −π + (2π/√2) = π ( (2/√2) − 1 ).
Since 2/√2 = √2, we obtain

  I = π (√2 − 1).

Thus the exact answer is

  I = π (√2 − 1).

A numerical approximation is: 
  π (√2 − 1) ≈ 3.1415926536 × (1.4142135624 − 1) ≈ 3.1415926536 × 0.4142135624 ≈ 1.3007025361.

Finally, we output the answer in the required JSON format.

{"answer": "$\\pi(\\sqrt{2}-1)$", "numerical_answer": "1.3007025361"}