To solve the definite integral \(\int_0^1 \frac{\ln\left(x + x^{-1}\right)}{x + x^{-1}} \, dx\), we will follow the steps outlined.

### Step 1: Analytical Solution

First, let's rewrite the integrand for clarity:
\[
\int_0^1 \frac{\ln\left(x + x^{-1}\right)}{x + x^{-1}} \, dx
\]

We can simplify the expression inside the logarithm:
\[
x + x^{-1} = x + \frac{1}{x} = \frac{x^2 + 1}{x}
\]

Thus, the integral becomes:
\[
\int_0^1 \frac{\ln\left(\frac{x^2 + 1}{x}\right)}{\frac{x^2 + 1}{x}} \, dx = \int_0^1 \frac{\ln(x^2 + 1) - \ln(x)}{\frac{x^2 + 1}{x}} \, dx
\]

Simplify the denominator:
\[
\frac{x^2 + 1}{x} = x + \frac{1}{x}
\]

So the integral is:
\[
\int_0^1 \frac{\ln(x^2 + 1) - \ln(x)}{x + \frac{1}{x}} \, dx
\]

Next, we make a substitution to simplify the integral. Let \( t = x + \frac{1}{x} \). Then:
\[
dt = \left(1 - \frac{1}{x^2}\right) dx
\]

However, this substitution is not straightforward to apply directly. Instead, we can use a different approach by recognizing a symmetry in the integral. Consider the substitution \( u = \frac{1}{x} \). Then \( du = -\frac{1}{x^2} dx \), and the limits of integration change from \( x = 0 \) to \( x = 1 \) to \( u = \infty \) to \( u = 1 \).

Rewriting the integral in terms of \( u \):
\[
\int_0^1 \frac{\ln\left(x + x^{-1}\right)}{x + x^{-1}} \, dx = \int_\infty^1 \frac{\ln\left(\frac{1}{u} + u\right)}{\frac{1}{u} + u} \left(-\frac{1}{u^2}\right) du
\]

Simplify the integrand:
\[
\int_\infty^1 \frac{\ln\left(u + \frac{1}{u}\right)}{u + \frac{1}{u}} \left(-\frac{1}{u^2}\right) du = \int_1^\infty \frac{\ln\left(u + \frac{1}{u}\right)}{u + \frac{1}{u}} \frac{1}{u^2} du
\]

Notice that the integrand is symmetric around \( x = 1 \). Therefore, we can combine the integrals:
\[
2 \int_0^1 \frac{\ln\left(x + x^{-1}\right)}{x + x^{-1}} \, dx = \int_0^\infty \frac{\ln\left(x + x^{-1}\right)}{x + x^{-1}} \, dx
\]

This integral is known to be:
\[
\int_0^\infty \frac{\ln\left(x + x^{-1}\right)}{x + x^{-1}} \, dx = \pi \ln 2
\]

Thus:
\[
2 \int_0^1 \frac{\ln\left(x + x^{-1}\right)}{x + x^{-1}} \, dx = \pi \ln 2
\]

So:
\[
\int_0^1 \frac{\ln\left(x + x^{-1}\right)}{x + x^{-1}} \, dx = \frac{\pi \ln 2}{2}
\]

### Step 2: Numerical Approximation

Using a numerical method or a calculator, we find:
\[
\frac{\pi \ln 2}{2} \approx 1.088793045
\]

### Step 3: JSON Format

\[
\boxed{
\begin{aligned}
&\text{"answer": "\frac{\pi \ln 2}{2}",} \\
&\text{"numerical_answer": "1.088793045"}
\end{aligned}
}
\]