To solve the definite integral \(\int_{0}^{1}{\frac{x^{3}+x+1}{3x^{2}-3x+4}}\:\mathrm{d}x\), we will follow the steps outlined:

### Step 1: Analytical Solution

First, we need to simplify the integrand \(\frac{x^{3}+x+1}{3x^{2}-3x+4}\). We can perform polynomial long division to simplify the fraction.

#### Polynomial Long Division

Divide \(x^3 + x + 1\) by \(3x^2 - 3x + 4\):

1. Divide the leading term of the numerator \(x^3\) by the leading term of the denominator \(3x^2\):
   \[
   \frac{x^3}{3x^2} = \frac{1}{3}x
   \]

2. Multiply \(\frac{1}{3}x\) by the entire denominator \(3x^2 - 3x + 4\):
   \[
   \frac{1}{3}x \cdot (3x^2 - 3x + 4) = x^3 - x^2 + \frac{4}{3}x
   \]

3. Subtract this result from the original numerator:
   \[
   (x^3 + x + 1) - (x^3 - x^2 + \frac{4}{3}x) = x^2 + \left(1 - \frac{4}{3}\right)x + 1 = x^2 - \frac{1}{3}x + 1
   \]

4. Now, divide the leading term of the new numerator \(x^2\) by the leading term of the denominator \(3x^2\):
   \[
   \frac{x^2}{3x^2} = \frac{1}{3}
   \]

5. Multiply \(\frac{1}{3}\) by the entire denominator \(3x^2 - 3x + 4\):
   \[
   \frac{1}{3} \cdot (3x^2 - 3x + 4) = x^2 - x + \frac{4}{3}
   \]

6. Subtract this result from the new numerator:
   \[
   (x^2 - \frac{1}{3}x + 1) - (x^2 - x + \frac{4}{3}) = \left(-\frac{1}{3}x + x\right) + \left(1 - \frac{4}{3}\right) = \frac{2}{3}x - \frac{1}{3}
   \]

So, the integrand can be written as:
\[
\frac{x^3 + x + 1}{3x^2 - 3x + 4} = \frac{1}{3}x + \frac{1}{3} + \frac{\frac{2}{3}x - \frac{1}{3}}{3x^2 - 3x + 4}
\]

Thus, the integral becomes:
\[
\int_{0}^{1} \left( \frac{1}{3}x + \frac{1}{3} + \frac{\frac{2}{3}x - \frac{1}{3}}{3x^2 - 3x + 4} \right) \, dx
\]

We can split this into three separate integrals:
\[
\int_{0}^{1} \frac{1}{3}x \, dx + \int_{0}^{1} \frac{1}{3} \, dx + \int_{0}^{1} \frac{\frac{2}{3}x - \frac{1}{3}}{3x^2 - 3x + 4} \, dx
\]

#### Evaluate the first two integrals:
\[
\int_{0}^{1} \frac{1}{3}x \, dx = \frac{1}{3} \int_{0}^{1} x \, dx = \frac{1}{3} \left[ \frac{x^2}{2} \right]_0^1 = \frac{1}{3} \cdot \frac{1}{2} = \frac{1}{6}
\]

\[
\int_{0}^{1} \frac{1}{3} \, dx = \frac{1}{3} \left[ x \right]_0^1 = \frac{1}{3} \cdot 1 = \frac{1}{3}
\]

#### Evaluate the third integral:
\[
\int_{0}^{1} \frac{\frac{2}{3}x - \frac{1}{3}}{3x^2 - 3x + 4} \, dx
\]

Let \(u = 3x^2 - 3x + 4\). Then \(du = (6x - 3) \, dx\). Notice that \(\frac{2}{3}x - \frac{1}{3} = \frac{1}{3}(2x - 1)\), so:
\[
\frac{2}{3}x - \frac{1}{3} = \frac{1}{3}(2x - 1) = \frac{1}{3} \cdot \frac{1}{2} (6x - 3) = \frac{1}{6} (6x - 3)
\]

Thus, the integral becomes:
\[
\int_{0}^{1} \frac{\frac{1}{6} (6x - 3)}{3x^2 - 3x + 4} \, dx = \frac{1}{6} \int_{0}^{1} \frac{6x - 3}{3x^2 - 3x + 4} \, dx = \frac{1}{6} \int_{0}^{1} \frac{du}{u}
\]

Since \(u = 3x^2 - 3x + 4\), we need to evaluate the limits of integration in terms of \(u\):
- When \(x = 0\), \(u = 4\)
- When \(x = 1\), \(u = 4\)

Thus, the integral becomes:
\[
\frac{1}{6} \int_{4}^{4} \frac{1}{u} \, du = 0
\]

### Step 2: Combine the Results

Combining all the results, we get:
\[
\int_{0}^{1} \frac{x^3 + x + 1}{3x^2 - 3x + 4} \, dx = \frac{1}{6} + \frac{1}{3} + 0 = \frac{1}{6} + \frac{2}{6} = \frac{3}{6} = \frac{1}{2}
\]

### Step 3: Numerical Approximation

The numerical approximation of \(\frac{1}{2}\) is:
\[
0.5000000000
\]

### Step 4: Output the Final Answer

\[
\boxed{
\begin{aligned}
\text{"answer": "}\frac{1}{2}\text{"}, \\
\text{"numerical_answer": "0.5000000000"}
\end{aligned}
}
\]