# Evaluating the Definite Integral

I'll calculate the definite integral:
$$\int_{0}^{2.0}x^{-1/2}(2.0-x)^{-1/2}\ln\left(1.0\sqrt{x(2.0-x)}+\sqrt{1+1.0^2x(2.0-x)}\right)dx$$

## Step 1: Simplify the expression
Let's denote $a = 1.0$ for clarity. The integral becomes:
$$\int_{0}^{2.0}x^{-1/2}(2.0-x)^{-1/2}\ln\left(a\sqrt{x(2.0-x)}+\sqrt{1+a^2x(2.0-x)}\right)dx$$

## Step 2: Apply substitution
Let's substitute $x = 2.0\sin^2(t)$, which gives $dx = 4.0\sin(t)\cos(t)dt$
When $x = 0$, $t = 0$, and when $x = 2.0$, $t = \frac{\pi}{2}$

Also, $2.0-x = 2.0(1-\sin^2(t)) = 2.0\cos^2(t)$

Therefore:
- $x^{-1/2} = (2.0\sin^2(t))^{-1/2} = \frac{1}{\sqrt{2.0}|\sin(t)|}$
- $(2.0-x)^{-1/2} = (2.0\cos^2(t))^{-1/2} = \frac{1}{\sqrt{2.0}|\cos(t)|}$
- $\sqrt{x(2.0-x)} = \sqrt{2.0\sin^2(t) \cdot 2.0\cos^2(t)} = 2.0|\sin(t)\cos(t)|$

Since we're in the first quadrant with $t \in [0, \frac{\pi}{2}]$, we can remove the absolute value signs.

## Step 3: Substitute into the integral
The expression becomes:
$$\int_{0}^{\frac{\pi}{2}} \frac{1}{\sqrt{2.0}\sin(t)} \cdot \frac{1}{\sqrt{2.0}\cos(t)} \cdot \ln(2.0a\sin(t)\cos(t) + \sqrt{1+4.0a^2\sin^2(t)\cos^2(t)}) \cdot 4.0\sin(t)\cos(t)dt$$

Simplifying:
$$\int_{0}^{\frac{\pi}{2}} 2.0 \cdot \ln(2.0a\sin(t)\cos(t) + \sqrt{1+4.0a^2\sin^2(t)\cos^2(t)})dt$$

Note that $\sin(t)\cos(t) = \frac{\sin(2t)}{2}$, so we get:
$$\int_{0}^{\frac{\pi}{2}} 2.0 \cdot \ln(a\sin(2t) + \sqrt{1+a^2\sin^2(2t)})dt$$

## Step 4: Apply a known result
This integral can be evaluated using the formula:
$$\int \ln(a\sin(u) + \sqrt{1+a^2\sin^2(u)})du = \ln\left(\frac{a+\sqrt{1+a^2}}{2}\right) \cdot u + \text{constant}$$

With $u = 2t$, we have $du = 2dt$, so:
$$\int \ln(a\sin(2t) + \sqrt{1+a^2\sin^2(2t)})dt = \frac{1}{2}\ln\left(\frac{a+\sqrt{1+a^2}}{2}\right) \cdot 2t + \text{constant} = \ln\left(\frac{a+\sqrt{1+a^2}}{2}\right) \cdot t + \text{constant}$$

## Step 5: Evaluate the definite integral
Applying the limits:
$$\int_{0}^{\frac{\pi}{2}} 2.0 \cdot \ln(a\sin(2t) + \sqrt{1+a^2\sin^2(2t)})dt = 2.0 \cdot \ln\left(\frac{a+\sqrt{1+a^2}}{2}\right) \cdot \left[\frac{\pi}{2} - 0\right]$$

$$= \pi \cdot \ln\left(\frac{a+\sqrt{1+a^2}}{2}\right)$$

## Step 6: Substitute back $a = 1.0$
$$= \pi \cdot \ln\left(\frac{1.0+\sqrt{1+1.0^2}}{2}\right) = \pi \cdot \ln\left(\frac{1+\sqrt{2}}{2}\right)$$

## Step 7: Calculate the numerical approximation
$$\pi \cdot \ln\left(\frac{1+\sqrt{2}}{2}\right) \approx 3.1415926536 \cdot \ln(0.8535533906) \approx 3.1415926536 \cdot (-0.1586215613) \approx -0.4982968539$$

The exact result is $\pi \cdot \ln\left(\frac{1+\sqrt{2}}{2}\right)$, and the numerical approximation is $-0.4982968539$.

{"answer": "\pi \cdot \ln\left(\frac{1+\sqrt{2}}{2}\right)", "numerical_answer": "-0.4982968539"}