Let's denote the integral as:
\[
I = \int_{1/\sqrt{2}}^1 \frac{\arcsin(x)}{x^3} \, dx
\]

**Step 1: Analytical Evaluation**

Let us use integration by parts:
Let \( u = \arcsin(x) \), \( dv = x^{-3} dx \).
Then \( du = \frac{1}{\sqrt{1-x^2}} dx \), \( v = \int x^{-3} dx = -\frac{1}{2}x^{-2} \).

By parts:
\[
I = uv\bigg|_{1/\sqrt{2}}^1 - \int_{1/\sqrt{2}}^1 v\, du
\]
\[
= \left[ \arcsin(x) \cdot \left(-\frac{1}{2}x^{-2}\right) \right]_{1/\sqrt{2}}^1 - \int_{1/\sqrt{2}}^1 \left(-\frac{1}{2} x^{-2}\right) \cdot \frac{1}{\sqrt{1-x^2}} dx
\]
\[
= -\frac{1}{2} \left[ \frac{\arcsin(x)}{x^2} \right]_{1/\sqrt{2}}^1 + \frac{1}{2} \int_{1/\sqrt{2}}^1 \frac{1}{x^2 \sqrt{1-x^2}} dx
\]

First term:
For \( x = 1 \): \( \arcsin(1) = \frac{\pi}{2}, x^2 = 1 \) ⇒ \( \frac{\arcsin(1)}{1^2} = \frac{\pi}{2} \)  
For \( x = \frac{1}{\sqrt{2}} \): \( \arcsin(1/\sqrt{2}) = \frac{\pi}{4}, x^2 = 1/2 \) ⇒ \( \frac{\arcsin(1/\sqrt{2})}{(1/\sqrt{2})^2} = \frac{\pi/4}{1/2} = \frac{\pi}{2} \)

Thus,
\[
\left[\frac{\arcsin(x)}{x^2}\right]_{1/\sqrt{2}}^1 = \frac{\pi}{2} - \frac{\pi}{2} = 0
\]
So,
\[
I = \frac{1}{2} \int_{1/\sqrt{2}}^1 \frac{1}{x^2 \sqrt{1-x^2}} dx
\]

**Step 2: Simplifying the Integral**

Let us focus on:
\[
J = \int_{1/\sqrt{2}}^1 \frac{1}{x^2 \sqrt{1-x^2}} dx
\]

Let \( x = \sin \theta \), so \( dx = \cos \theta\, d\theta \), \( \sqrt{1 - x^2} = \cos \theta \).

For \( x = 1/\sqrt{2} \), \( \sin\theta_0 = 1/\sqrt{2} \implies \theta_0 = \frac{\pi}{4} \).  
For \( x = 1 \), \( \theta_1 = \frac{\pi}{2} \).

Change of variables:
- \( x = \sin\theta \), \( dx = \cos\theta\, d\theta \)
- \( x^2 = \sin^2\theta \)
- \( \sqrt{1 - x^2} = \cos\theta \)

So,
\[
J = \int_{\pi/4}^{\pi/2} \frac{1}{\sin^2\theta \cos\theta} \cdot \cos\theta\, d\theta = \int_{\pi/4}^{\pi/2} \csc^2\theta\, d\theta
\]
\[
\csc^2\theta = \frac{1}{\sin^2\theta}
\]
\[
\int \csc^2\theta\, d\theta = -\cot\theta + C
\]
So,
\[
J = \left[-\cot\theta\right]_{\pi/4}^{\pi/2} = -\cot\left(\frac{\pi}{2}\right) + \cot\left(\frac{\pi}{4}\right)
\]

Now,
- \( \cot(\frac{\pi}{2}) = 0 \)
- \( \cot(\frac{\pi}{4}) = 1 \)

So,
\[
J = -0 + 1 = 1
\]
Therefore,
\[
I = \frac{1}{2}(1) = \frac{1}{2}
\]

**Step 3: Numerical Approximation**

\[
I \approx 0.5
\]

**Step 4: JSON Format**

```json
{"answer": "\\frac{1}{2}", "numerical_answer": "0.5000000000"}
```