We start with the given integral

  I = ∫₁^(e^e) (log(x^(log(x^x))) / x²) dx.

Step 1. Simplify the numerator.
  Notice that
    log(x^(log(x^x))) = log(x) · log(x^x).
  Since log(x^x) = x · log(x), we have
    log(x^(log(x^x))) = log(x) · [x · log(x)] = x · (log(x))².

Thus the integrand becomes
  [x · (log(x))²] / x² = (log(x))² / x.

Step 2. Change of variables.
  Let u = log(x) so that du = (1/x) dx, or equivalently dx = x du.
  Changing the integral gives:
    I = ∫ (u²/x) · (x du) = ∫ u² du.
  The new limits:
    when x = 1, u = log(1) = 0;
    when x = e^e, u = log(e^e) = e.

Step 3. Evaluate the simplified integral.
  I = ∫₀^(e) u² du = [u³/3] evaluated from 0 to e = (e³/3) - 0 = e³/3.

Step 4. Numerical approximation.
  Using the approximate value e ≈ 2.7182818285, we compute:
    e³ ≈ 2.7182818285³ ≈ 20.0855369232,
    so that I ≈ 20.0855369232/3 ≈ 6.6951789744.

The final answers are:

{"answer": "\\frac{e^3}{3}", "numerical_answer": "6.6951789744"}