To solve the definite integral \(\int\limits_0^1 x^{-1} \ln x \ln \frac{2+x}{2-x} \, dx\), we will follow the steps outlined.

### Step 1: Analytical Computation

First, let's rewrite the integral for clarity:
\[ I = \int_0^1 \frac{\ln x \ln \frac{2+x}{2-x}}{x} \, dx. \]

We can use the series expansion for \(\ln \frac{2+x}{2-x}\):
\[ \ln \frac{2+x}{2-x} = \ln \left(1 + \frac{x}{2}\right) - \ln \left(1 - \frac{x}{2}\right). \]

Using the Taylor series for \(\ln(1 + y)\) and \(\ln(1 - y)\):
\[ \ln(1 + y) = \sum_{n=1}^\infty \frac{(-1)^{n+1} y^n}{n}, \]
\[ \ln(1 - y) = -\sum_{n=1}^\infty \frac{y^n}{n}. \]

Thus,
\[ \ln \frac{2+x}{2-x} = \sum_{n=1}^\infty \frac{(-1)^{n+1} \left(\frac{x}{2}\right)^n}{n} + \sum_{n=1}^\infty \frac{\left(\frac{x}{2}\right)^n}{n}. \]

Combining these series:
\[ \ln \frac{2+x}{2-x} = \sum_{n=1}^\infty \frac{(-1)^{n+1} + 1}{n} \left(\frac{x}{2}\right)^n. \]

Since \((-1)^{n+1} + 1\) is 2 for odd \(n\) and 0 for even \(n\), we can simplify this to:
\[ \ln \frac{2+x}{2-x} = 2 \sum_{k=0}^\infty \frac{1}{2k+1} \left(\frac{x}{2}\right)^{2k+1}. \]

Now, substitute this back into the integral:
\[ I = \int_0^1 \frac{\ln x}{x} \cdot 2 \sum_{k=0}^\infty \frac{1}{2k+1} \left(\frac{x}{2}\right)^{2k+1} \, dx. \]

Interchange the sum and the integral:
\[ I = 2 \sum_{k=0}^\infty \frac{1}{2k+1} \int_0^1 \frac{\ln x}{x} \left(\frac{x}{2}\right)^{2k+1} \, dx. \]

Simplify the integrand:
\[ I = 2 \sum_{k=0}^\infty \frac{1}{2k+1} \int_0^1 \ln x \cdot \frac{x^{2k}}{2^{2k+1}} \, dx. \]

Factor out the constants:
\[ I = 2 \sum_{k=0}^\infty \frac{1}{2k+1} \cdot \frac{1}{2^{2k+1}} \int_0^1 x^{2k} \ln x \, dx. \]

The integral \(\int_0^1 x^{2k} \ln x \, dx\) can be evaluated using integration by parts. Let \(u = \ln x\) and \(dv = x^{2k} dx\). Then \(du = \frac{1}{x} dx\) and \(v = \frac{x^{2k+1}}{2k+1}\). Thus,
\[ \int_0^1 x^{2k} \ln x \, dx = \left[ \frac{x^{2k+1} \ln x}{2k+1} \right]_0^1 - \int_0^1 \frac{x^{2k+1}}{2k+1} \cdot \frac{1}{x} \, dx. \]

The boundary term evaluates to 0, and the remaining integral is:
\[ \int_0^1 x^{2k} \ln x \, dx = -\frac{1}{(2k+1)^2}. \]

Substitute this back into the series:
\[ I = 2 \sum_{k=0}^\infty \frac{1}{2k+1} \cdot \frac{1}{2^{2k+1}} \cdot \left(-\frac{1}{(2k+1)^2}\right). \]

Simplify:
\[ I = -2 \sum_{k=0}^\infty \frac{1}{(2k+1)^3 2^{2k+1}}. \]

This series can be recognized as a known series representation of the Catalan constant \(G\):
\[ G = \sum_{k=0}^\infty \frac{(-1)^k}{(2k+1)^2}. \]

Thus, the integral evaluates to:
\[ I = -2 \cdot \frac{G}{2} = -G. \]

### Step 2: Numerical Approximation

The Catalan constant \(G\) is approximately:
\[ G \approx 0.915965594177219015054603514932384110774. \]

Thus, the numerical approximation of the integral is:
\[ I \approx -0.915965594177219015054603514932384110774. \]

### Step 3: Final Answer in JSON Format

```json
{"answer": "-G", "numerical_answer": "-0.915965594177219015054603514932384110774"}
```