Let’s tackle the integral step by step:

\[
I = \int_{0}^{1} x \sqrt{1^2 - x^2} \arcsin(0.5x) dx = \int_{0}^{1} x \sqrt{1 - x^2} \arcsin(0.5x) dx
\]

**Step 1: Substitution**

Let \( x = \sin\theta \), where \( \theta \in [0, \frac{\pi}{2}] \).

Then:
- \( dx = \cos\theta \, d\theta \)
- \( \sqrt{1 - x^2} = \sqrt{1 - \sin^2\theta} = \cos\theta \)
- \( x = \sin\theta \)
- When \( x=0 \) ⇒ \( \theta = 0 \)
- When \( x=1 \) ⇒ \( \theta = \frac{\pi}{2} \)
- \( \arcsin(0.5x) = \arcsin(0.5\sin\theta) \)

Thus, the integral becomes

\[
I = \int_{0}^{\frac{\pi}{2}} \sin\theta \cdot \cos\theta \cdot \arcsin(0.5\sin\theta) \cdot \cos\theta \; d\theta = \int_{0}^{\frac{\pi}{2}} \sin\theta \cos^2\theta \arcsin(0.5\sin\theta) \; d\theta
\]

**Step 2: Integration by parts**

Let
- \( u = \arcsin(0.5\sin\theta) \Rightarrow du = \frac{0.5\cos\theta}{\sqrt{1-(0.5\sin\theta)^2}} d\theta \)
- \( dv = \sin\theta \cos^2\theta \, d\theta \)

Let’s compute \( v \):

\[
dv = \sin\theta \cos^2\theta d\theta
\]

Let’s compute this integral separately:

Let \( w = \cos\theta \Longrightarrow dw = -\sin\theta d\theta \),
so \(\sin\theta d\theta = -dw\),
therefore

\[
\int \sin\theta \cos^2\theta d\theta = -\int w^2 dw = -\frac{w^3}{3} = -\frac{\cos^3\theta}{3}
\]

So \( v = -\frac{\cos^3\theta}{3} \).

Now, by integration by parts:

\[
I = uv\Big|_{0}^{\frac{\pi}{2}} - \int_{0}^{\frac{\pi}{2}} v du
\]
\[
I = \left[ \arcsin(0.5\sin\theta) \left(-\frac{\cos^3\theta}{3}\right) \right]_{0}^{\frac{\pi}{2}} + \frac{1}{3} \int_{0}^{\frac{\pi}{2}} \cos^3\theta \cdot \frac{0.5\cos\theta}{\sqrt{1-0.25\sin^2\theta}} d\theta
\]
\[
= \left[ -\frac{1}{3} \arcsin(0.5\sin\theta) \cos^3\theta \right]_{0}^{\frac{\pi}{2}} + \frac{1}{6} \int_{0}^{\frac{\pi}{2}} \frac{\cos^4\theta}{\sqrt{1-0.25\sin^2\theta}} d\theta
\]

Let’s look at the boundary term first:

For \(\theta = 0\): \( \arcsin(0.5\cdot 0) = 0 \); \( \cos^3 0 = 1 \), so term is 0.

For \(\theta = \frac{\pi}{2}\): \( \arcsin(0.5\cdot 1) = \arcsin(0.5) = \frac{\pi}{6} \); \( \cos(\frac{\pi}{2}) = 0 \), so term is 0.

Thus boundary term is 0 - 0 = 0.

So:

\[
I = \frac{1}{6} \int_{0}^{\frac{\pi}{2}} \frac{\cos^4\theta}{\sqrt{1-0.25\sin^2\theta}} d\theta
\]

**Step 3: Express \(\cos^4 \theta\) in terms of cosines of multiples of \(\theta\)**

\[
\cos^4 \theta = \left(\cos^2 \theta\right)^2 = \left(\frac{1 + \cos 2\theta}{2}\right)^2 = \frac{1}{4} (1 + 2\cos 2\theta + \cos^2 2\theta)
\]
Now,
\[
\cos^2 2\theta = \frac{1 + \cos 4\theta}{2}
\]
So
\[
\cos^4 \theta = \frac{1}{4} (1 + 2\cos 2\theta + \frac{1 + \cos 4\theta}{2}) = \frac{1}{4}\left(1 + 2\cos 2\theta + \frac{1}{2} + \frac{1}{2}\cos 4\theta\right)
\]
\[
= \frac{1}{4}\left(\frac{3}{2} + 2\cos 2\theta + \frac{1}{2}\cos 4\theta\right) = \frac{3}{8} + \frac{1}{2} \cos 2\theta + \frac{1}{8} \cos 4\theta
\]

So

\[
I = \frac{1}{6} \int_{0}^{\frac{\pi}{2}} \frac{3/8 + 1/2\cos 2\theta + 1/8\cos 4\theta}{\sqrt{1-0.25\sin^2\theta}} d\theta
\]
\[
= \frac{1}{6}\left[\frac{3}{8} \int_{0}^{\frac{\pi}{2}} \frac{d\theta}{\sqrt{1-0.25\sin^2\theta}}
+ \frac{1}{2} \int_{0}^{\frac{\pi}{2}} \frac{\cos 2\theta\, d\theta}{\sqrt{1-0.25\sin^2\theta}}
+ \frac{1}{8} \int_{0}^{\frac{\pi}{2}} \frac{\cos 4\theta d\theta}{\sqrt{1-0.25\sin^2\theta}}
\right]
\]

Let's denote \( k = 0.5 \). The denominator is \( \sqrt{1 - k^2 \sin^2\theta} \).

Let’s relate these with standard forms of elliptic integrals:

\[
F(\phi, k) = \int_0^\phi \frac{d\theta}{\sqrt{1 - k^2 \sin^2 \theta}}
\]
\[
E(\phi, k) = \int_0^\phi \sqrt{1 - k^2 \sin^2 \theta} \, d\theta
\]

For the integrals with cosines in the numerator, we use known relations:

\[
\int_0^{\frac{\pi}{2}} \frac{\cos(n\theta)}{\sqrt{1 - k^2 \sin^2 \theta}} d\theta = ?
\]
These are called the elliptic integrals of the third kind if \(\cos n\theta\) is replaced by more general functions, but otherwise can be related to the derivatives or recurrences involving elliptic integrals.

But let's try to relate the integrals term-by-term.

- The first term:

\[
I_1 = \int_0^{\frac{\pi}{2}} \frac{d\theta}{\sqrt{1 - k^2 \sin^2 \theta}} = K(k)
\]

where \( K(k) \) is the complete elliptic integral of the first kind.

- The second term:

\[
I_2 = \int_0^{\frac{\pi}{2}} \frac{\cos 2\theta \, d\theta}{\sqrt{1 - k^2 \sin^2 \theta}}
\]

But since \( \cos 2\theta = 1 - 2\sin^2\theta \), then

\[
I_2 = \int_0^{\frac{\pi}{2}} \frac{d\theta}{\sqrt{1 - k^2 \sin^2 \theta}} - 2\int_0^{\frac{\pi}{2}} \frac{\sin^2\theta\, d\theta}{\sqrt{1 - k^2 \sin^2 \theta}}
\]

Let

\[
J = \int_0^{\frac{\pi}{2}} \frac{\sin^2\theta\, d\theta}{\sqrt{1 - k^2 \sin^2 \theta}}
\]

It is known that

\[
J = \frac{1}{k^2} \left( E(k) - (1 - k^2) K(k) \right)
\]

where \( E(k) \) is the complete elliptic integral of the second kind.

So,

\[
I_2 = K(k) - 2J = K(k) - \frac{2}{k^2} \left( E(k) - (1 - k^2) K(k) \right ) = \frac{2(1-k^2)}{k^2}K(k) - \frac{2}{k^2}E(k) + K(k)
\]
\[
= \left( \frac{2(1-k^2)}{k^2} + 1 \right) K(k) - \frac{2}{k^2} E(k)
\]
\[
= \left( \frac{2 - 2k^2 + k^2}{k^2} \right) K(k) - \frac{2}{k^2} E(k)
= \frac{2 - k^2}{k^2} K(k) - \frac{2}{k^2} E(k)
\]

Plug in \( k = 0.5 \implies k^2 = 0.25 \):

\[
\frac{2 - 0.25}{0.25} = \frac{1.75}{0.25} = 7
\]

So,

\[
I_2 = 7 K(k) - 8 E(k)
\]

Similarly, for the third term:

\[
I_3 = \int_0^{\frac{\pi}{2}} \frac{\cos 4\theta\, d\theta}{\sqrt{1 - k^2 \sin^2\theta}}
\]

We can use \( \cos 4\theta = 1 - 8 \sin^2\theta + 8 \sin^4\theta \):

\[
\cos 4\theta = 1 - 8 \sin^2\theta + 8 \sin^4\theta
\]

So,

\[
I_3 = \int_0^{\frac{\pi}{2}} \frac{d\theta}{\sqrt{1 - k^2 \sin^2\theta}} - 8\int_0^{\frac{\pi}{2}} \frac{\sin^2\theta d\theta}{\sqrt{1 - k^2 \sin^2\theta}} + 8\int_0^{\frac{\pi}{2}} \frac{\sin^4\theta\, d\theta}{\sqrt{1 - k^2 \sin^2\theta}}
\]

We already have \( J \) from before. Let’s denote

\[
K = \int_0^{\frac{\pi}{2}} \frac{\sin^4\theta\, d\theta}{\sqrt{1 - k^2 \sin^2\theta}}
\]

Now, the general formula for \( n\geq0 \):

\[
\int_0^{\frac{\pi}{2}} \frac{\sin^{2n}\theta}{\sqrt{1 - k^2 \sin^2\theta}} d\theta = S_n(k)
\]

For \( n = 2 \):

\[
S_2(k) = \frac{1}{3k^4} [(2+k^2)E(k) - 2(1 - k^2)K(k)]
\]

Thus,

\[
K = S_2(k) = \frac{1}{3k^4}\left[(2 + k^2) E(k) - 2(1 - k^2) K(k)\right]
\]

Plugging in \( k = 0.5, k^2=0.25, k^4 = 0.0625 \):

- \( 2+k^2 = 2.25 \)
- \( 2(1-k^2) = 2(0.75) = 1.5 \)
- \( 3k^4 = 0.1875 \)

So

\[
K = \frac{1}{0.1875}(2.25 E(k) - 1.5 K(k))
\]

Now, putting together,

\[
I_3 = K(k) - 8 J + 8 K
\]

Recall \( J = \frac{1}{k^2}(E(k)-(1 - k^2)K(k)) \), so with \( k^2 = 0.25 \):

\[
J = 4 (E(k) - 0.75 K(k))
\]

Let’s compute \( I_3 \):

\(
I_3 = K(k) - 8 \times 4(E(k) - 0.75 K(k)) + 8 \times \frac{1}{0.1875}(2.25 E(k) - 1.5 K(k))
\)
\(
= K(k) - 32 E(k) + 24 K(k) + \frac{8}{0.1875}(2.25 E(k) - 1.5 K(k))
\)
But actually, more simply,
\(
I_3 =
K(k) - 32 E(k) + 24 K(k) +
\frac{8 \cdot 2.25}{0.1875} E(k) -
\frac{8 \cdot 1.5}{0.1875} K(k)
\)

Compute \( \frac{8}{0.1875} = \frac{8 \times 8}{1.5} = \frac{64}{1.5} = 42.666... \)
Therefore,

\[
I_3 = K(k) - 32 E(k) + 24 K(k) + 95.99999 E(k) - 64 K(k)
\]
Sum \( K(k): 1 + 24 - 64 = -39 \)
Sum \( E(k): -32 + 95.99999 = 63.99999 \)

Thus,

\[
I_3 = -39 K(k) + 64 E(k)
\]

**Summary**

Now, plug the results \(k=0.5\) into our earlier sum:

\[
I = \frac{1}{6}\left[
\frac{3}{8} K(k)
+ \frac{1}{2} I_2
+ \frac{1}{8} I_3
\right]
\]

Recall:
- \( I_2 = 7 K(k) - 8 E(k) \)
- \( I_3 = -39 K(k) + 64 E(k) \)

So:

\[
I = \frac{1}{6} \left[
\frac{3}{8}K
+ \frac{1}{2}(7K - 8E)
+ \frac{1}{8}(-39K + 64E)
\right]
\]
\[
= \frac{1}{6} \left[
\frac{3}{8} K + \frac{7}{2} K - 4 E
- \frac{39}{8} K + 8 E
\right]
\]

Combine K terms:

\[
\frac{3}{8} + \frac{7}{2} - \frac{39}{8}
\]
First, convert all to eighths:
\(
\frac{3}{8} + \frac{28}{8} - \frac{39}{8} = \frac{(3 + 28 - 39)}{8} = \frac{-8}{8} = -1
\)

E terms: \( -4 E + 8 E = 4 E \)

So,

\[
I = \frac{1}{6} ( - K(k) + 4 E(k) )
\]

Thus, the answer is:

\[
I = \frac{1}{6} \left( 4 E\left(\frac{1}{2}\right) - K\left(\frac{1}{2}\right) \right)
\]

**Step 4: Numerical Evaluation**

Values from tables or computational tools:

- \( K(0.5) \approx 1.6857503548 \)
- \( E(0.5) \approx 1.4674622093 \)

So,

\[
I \approx \frac{1}{6} ( 4 \times 1.4674622093 - 1.6857503548 )
= \frac{1}{6} (5.8698488372 - 1.6857503548 )
= \frac{1}{6} (4.1840984824 )
\approx 0.6973497471
\]

**JSON format:**

```json
{"answer": "\\frac{1}{6} \\left( 4\\, E\\left(\\frac{1}{2}\\right) - K\\left(\\frac{1}{2}\\right) \\right)", "numerical_answer": "0.6973497471"}
```