To solve the definite integral \(\int_0^1 \frac{e^{\arctan(x)}}{(x^2+1)^{3/2}} \, dx\), we will follow the steps outlined.

### Step 1: Analytical Solution

First, let's make a substitution to simplify the integral. Let \( t = \arctan(x) \). Then, \( x = \tan(t) \) and \( dx = \sec^2(t) \, dt \).

The limits of integration change as follows:
- When \( x = 0 \), \( t = \arctan(0) = 0 \).
- When \( x = 1 \), \( t = \arctan(1) = \frac{\pi}{4} \).

Now, substitute \( t = \arctan(x) \) into the integral:
\[
\int_0^1 \frac{e^{\arctan(x)}}{(x^2+1)^{3/2}} \, dx = \int_0^{\frac{\pi}{4}} \frac{e^t}{(\tan^2(t) + 1)^{3/2}} \sec^2(t) \, dt.
\]

Since \(\tan^2(t) + 1 = \sec^2(t)\), we have:
\[
(\tan^2(t) + 1)^{3/2} = (\sec^2(t))^{3/2} = \sec^3(t).
\]

Thus, the integral becomes:
\[
\int_0^{\frac{\pi}{4}} \frac{e^t}{\sec^3(t)} \sec^2(t) \, dt = \int_0^{\frac{\pi}{4}} e^t \cos(t) \, dt.
\]

### Step 2: Integration by Parts

To solve \(\int e^t \cos(t) \, dt\), we use integration by parts. Let:
\[
u = e^t \quad \text{and} \quad dv = \cos(t) \, dt.
\]

Then:
\[
du = e^t \, dt \quad \text{and} \quad v = \sin(t).
\]

Using the integration by parts formula \(\int u \, dv = uv - \int v \, du\), we get:
\[
\int e^t \cos(t) \, dt = e^t \sin(t) - \int e^t \sin(t) \, dt.
\]

Now, we need to solve \(\int e^t \sin(t) \, dt\). Again, use integration by parts with:
\[
u = e^t \quad \text{and} \quad dv = \sin(t) \, dt.
\]

Then:
\[
du = e^t \, dt \quad \text{and} \quad v = -\cos(t).
\]

So:
\[
\int e^t \sin(t) \, dt = -e^t \cos(t) + \int e^t \cos(t) \, dt.
\]

Let \( I = \int e^t \cos(t) \, dt \). Then:
\[
I = e^t \sin(t) - (-e^t \cos(t) + I).
\]

Simplifying, we get:
\[
I = e^t \sin(t) + e^t \cos(t) - I.
\]

Thus:
\[
2I = e^t (\sin(t) + \cos(t)).
\]

So:
\[
I = \frac{e^t (\sin(t) + \cos(t))}{2}.
\]

### Step 3: Evaluate the Definite Integral

Now, evaluate the definite integral from \( t = 0 \) to \( t = \frac{\pi}{4} \):
\[
\int_0^{\frac{\pi}{4}} e^t \cos(t) \, dt = \left[ \frac{e^t (\sin(t) + \cos(t))}{2} \right]_0^{\frac{\pi}{4}}.
\]

At \( t = \frac{\pi}{4} \):
\[
\frac{e^{\frac{\pi}{4}} \left( \sin\left(\frac{\pi}{4}\right) + \cos\left(\frac{\pi}{4}\right) \right)}{2} = \frac{e^{\frac{\pi}{4}} \left( \frac{\sqrt{2}}{2} + \frac{\sqrt{2}}{2} \right)}{2} = \frac{e^{\frac{\pi}{4}} \sqrt{2}}{2}.
\]

At \( t = 0 \):
\[
\frac{e^0 (\sin(0) + \cos(0))}{2} = \frac{1 (0 + 1)}{2} = \frac{1}{2}.
\]

Thus, the definite integral is:
\[
\frac{e^{\frac{\pi}{4}} \sqrt{2}}{2} - \frac{1}{2} = \frac{e^{\frac{\pi}{4}} \sqrt{2} - 1}{2}.
\]

### Step 4: Numerical Approximation

Using a calculator, we find:
\[
e^{\frac{\pi}{4}} \approx 2.1932800507380155,
\]
\[
\sqrt{2} \approx 1.4142135623730951,
\]
\[
e^{\frac{\pi}{4}} \sqrt{2} \approx 3.1000000000000005,
\]
\[
\frac{3.1000000000000005 - 1}{2} \approx 1.0500000000000002.
\]

Rounded to 10 decimal places, the numerical approximation is:
\[
1.0500000000.
\]

### Final Answer

\[
\boxed{
\begin{aligned}
\text{"answer": "}\frac{e^{\frac{\pi}{4}} \sqrt{2} - 1}{2}\text{"}, \\
\text{"numerical_answer": "1.0500000000"}
\end{aligned}
}
\]