We wish to evaluate

  I = ∫₀² x^(–1/2)(2 – x)^(–1/2) cos(√(x(2 – x))) dx.

Step 1. Substitution

Let
  x = 2 sin²θ.
Then
  dx = 4 sinθ cosθ dθ.
Also, note:
  2 – x = 2 – 2 sin²θ = 2 cos²θ.

The factors in the integrand become:
  x^(–1/2) = 1/√(2 sin²θ) = 1/(√2 sinθ),
  (2 – x)^(–1/2) = 1/√(2 cos²θ) = 1/(√2 cosθ).

Thus,
  x^(–1/2)(2 – x)^(–1/2) = 1/((√2 sinθ)(√2 cosθ)) = 1/(2 sinθ cosθ).

Also, observe that
  √(x(2 – x)) = √(2 sin²θ · 2 cos²θ) = 2 sinθ cosθ.

Therefore, the integrand along with dx becomes:
  [1/(2 sinθ cosθ)] · cos(2 sinθ cosθ) · [4 sinθ cosθ dθ] = 2 cos(2 sinθ cosθ) dθ.

Next, change the integration limits:
  When x = 0: 2 sin²θ = 0  ⟹ θ = 0.
  When x = 2: 2 sin²θ = 2  ⟹ sin²θ = 1 ⟹ θ = π/2.

Thus, the integral is transformed into:
  I = 2 ∫₀^(π/2) cos(2 sinθ cosθ) dθ.

Step 2. Simplify the integrand

Recall that
  2 sinθ cosθ = sin(2θ).
Thus, the integral becomes:
  I = 2 ∫₀^(π/2) cos(sin2θ) dθ.

Now, we perform a further substitution:
  Let u = 2θ ⟹ du = 2 dθ ⟹ dθ = du/2.
When θ = 0, u = 0; when θ = π/2, u = π.
Substituting, we get:
  I = 2 ∫₀^π cos(sin u) (du/2) = ∫₀^π cos(sin u) du.

Step 3. Recognize a standard Bessel integral

A well-known integral representation for the Bessel function J₀ is:
  J₀(z) = (1/π) ∫₀^π cos(z sin u) du.
Taking z = 1 we have:
  ∫₀^π cos(sin u) du = π J₀(1).

Thus, the exact value of the original integral is:
  I = π J₀(1).

Step 4. Numerical approximation

We know that the Bessel function of zero order at 1 is approximately:
  J₀(1) ≈ 0.7651976866.
Thus,
  I ≈ π × 0.7651976866 ≈ 2.4041138066.

Final Answer in JSON Format:
{"answer": "\\pi J_{0}(1)", "numerical_answer": "2.4041138066"}