To evaluate the definite integral

$$
\int_0^1 \frac{x - 1}{(x + 1)\ln x} \, dx,
$$

we begin by recognizing that the integrand involves both $ \ln x $ and a rational function of $ x $, which suggests the use of known integral identities or transformations involving logarithmic functions.

---

### Step 1: Use of a Known Identity

We apply the identity:

$$
\frac{x - 1}{\ln x} = \int_0^1 x^a \, da.
$$

This identity allows us to rewrite the integrand as:

$$
\frac{x - 1}{(x + 1)\ln x} = \int_0^1 \frac{x^a}{x + 1} \, da.
$$

Substituting into the original integral:

$$
\int_0^1 \frac{x - 1}{(x + 1)\ln x} \, dx = \int_0^1 \left( \int_0^1 \frac{x^a}{x + 1} \, da \right) dx.
$$

By Fubiniâ€™s Theorem, we can interchange the order of integration:

$$
= \int_0^1 \left( \int_0^1 \frac{x^a}{x + 1} \, dx \right) da.
$$

---

### Step 2: Evaluate the Inner Integral

Let us define:

$$
I(a) = \int_0^1 \frac{x^a}{x + 1} \, dx.
$$

This integral can be evaluated using a power series expansion of $ \frac{1}{x + 1} $:

$$
\frac{1}{x + 1} = \sum_{k=0}^\infty (-1)^k x^k \quad \text{for } 0 < x < 1.
$$

Then:

$$
I(a) = \int_0^1 x^a \sum_{k=0}^\infty (-1)^k x^k \, dx = \sum_{k=0}^\infty (-1)^k \int_0^1 x^{a + k} \, dx = \sum_{k=0}^\infty \frac{(-1)^k}{a + k + 1}.
$$

Now, integrate $ I(a) $ over $ a \in [0,1] $:

$$
\int_0^1 I(a) \, da = \sum_{k=0}^\infty (-1)^k \int_0^1 \frac{1}{a + k + 1} \, da = \sum_{k=0}^\infty (-1)^k \ln\left(\frac{k + 2}{k + 1}\right).
$$

This is a telescoping alternating series:

$$
\sum_{k=0}^\infty (-1)^k \ln\left(\frac{k + 2}{k + 1}\right) = \ln\left(\frac{2}{1}\right) - \ln\left(\frac{3}{2}\right) + \ln\left(\frac{4}{3}\right) - \ln\left(\frac{5}{4}\right) + \cdots
$$

Grouping terms:

$$
= \ln(2) - \ln\left(\frac{3}{2}\right) + \ln\left(\frac{4}{3}\right) - \ln\left(\frac{5}{4}\right) + \cdots
$$

This simplifies to:

$$
\sum_{k=0}^\infty (-1)^k \ln\left(\frac{k + 2}{k + 1}\right) = \ln\left(\frac{\pi}{2}\right),
$$

which is a known result derived from the properties of the Dirichlet eta function and its relation to the Riemann zeta function.

---

### Step 3: Final Result

Thus, the value of the definite integral is:

$$
\int_0^1 \frac{x - 1}{(x + 1)\ln x} \, dx = \ln\left(\frac{\pi}{2}\right).
$$

A numerical approximation of this value is:

$$
\ln\left(\frac{\pi}{2}\right) \approx 0.4515827052.
$$

---

### Final Answer

$$
\boxed{
\left\{
  "answer": "\\ln\\left(\\frac{\\pi}{2}\\