Let's compute the integral:
\[
I = \int_0^{0.5} x(0.5^2 - x^2)^{-1/2} \arcsin(0.5x) \, dx
\]

**Step 1: Substitution**

Let’s use the substitution:
\[
x = 0.5 \sin\theta \implies dx = 0.5 \cos\theta\, d\theta
\]
As \(x\) goes from \(0\) to \(0.5\):
- When \(x = 0: \sin\theta = 0 \implies \theta = 0\)
- When \(x = 0.5: \sin\theta = 1 \implies \theta = \frac{\pi}{2}\)

Calculate \((0.5^2 - x^2)^{-1/2}\):
\[
0.5^2 - x^2 = 0.25 - 0.25\sin^2\theta = 0.25(1 - \sin^2\theta) = 0.25\cos^2\theta
\]
\[
(0.5^2 - x^2)^{-1/2} = (0.25 \cos^2\theta)^{-1/2} = 2 \sec\theta
\]

Also,
\[
x = 0.5 \sin\theta
\]
\[
0.5x = 0.25\sin\theta
\]
\[
\arcsin(0.5x) = \arcsin(0.25\sin\theta)
\]

Substitute everything:
\[
I = \int_{0}^{\frac{\pi}{2}} [0.5 \sin\theta][2\sec\theta]\arcsin(0.25\sin\theta)[0.5\cos\theta] d\theta
\]
\[
= \int_{0}^{\frac{\pi}{2}} 0.5 \cdot 2 \cdot 0.5 \sin\theta \sec\theta \arcsin(0.25\sin\theta)\cos\theta\, d\theta
\]
\[
= 0.5 \int_{0}^{\frac{\pi}{2}} \sin\theta \sec\theta \arcsin(0.25\sin\theta)\cos\theta \, d\theta
\]
Note that \(\sec\theta \cos\theta = 1\). Therefore,
\[
I = 0.5 \int_0^{\frac{\pi}{2}} \sin\theta \arcsin(0.25\sin\theta) d\theta
\]

**Step 2: Using Integral by Parts**

Let \(u = \arcsin(0.25\sin\theta)\), \(dv = \sin\theta d\theta\), so \(du = \frac{0.25\cos\theta}{\sqrt{1-(0.25\sin\theta)^2}} d\theta\), and \(v = -\cos\theta\).

Using integration by parts:
\[
\int u\, dv = uv - \int v\, du
\]
So,
\[
I = 0.5 \left\{ -\cos\theta \arcsin(0.25\sin\theta) \Big|_0^{\frac{\pi}{2}} + \int_0^{\frac{\pi}{2}} \cos\theta \cdot \frac{0.25\cos\theta}{\sqrt{1-0.0625\sin^2\theta}} d\theta \right\}
\]
\[
= 0.5 \left\{ -\cos\theta \arcsin(0.25\sin\theta) \Big|_0^{\frac{\pi}{2}} + 0.25\int_0^{\frac{\pi}{2}} \frac{\cos^2\theta}{\sqrt{1-0.0625\sin^2\theta}} d\theta \right\}
\]

Compute the boundary term:
- At \(\theta = \frac{\pi}{2}\): \(\cos\theta = 0\), so term is 0.
- At \(\theta = 0\): \(\cos\theta = 1, \sin\theta = 0 \implies \arcsin(0)=0\), so term is 0.

Therefore, the boundary term is zero.

So,
\[
I = 0.5 \times 0.25 \int_0^{\frac{\pi}{2}} \frac{\cos^2\theta}{\sqrt{1-0.0625\sin^2\theta}} d\theta
= 0.125 \int_0^{\frac{\pi}{2}} \frac{\cos^2\theta}{\sqrt{1-0.0625\sin^2\theta}} d\theta
\]

**Step 3: Simplifying the Integral**

Recall:
\[
\cos^2\theta = 1 - \sin^2\theta
\]
So,
\[
I = 0.125 \int_0^{\frac{\pi}{2}} \frac{1 - \sin^2\theta}{\sqrt{1 - 0.0625\sin^2\theta}} d\theta
= 0.125 \left(
\int_0^{\frac{\pi}{2}} \frac{d\theta}{\sqrt{1 - 0.0625\sin^2\theta}}
- \int_0^{\frac{\pi}{2}} \frac{\sin^2\theta\, d\theta}{\sqrt{1 - 0.0625\sin^2\theta}}
\right)
\]

**Step 4: Express in terms of Elliptic Integrals**

We use the complete elliptic integrals of the first and second kind, defined as:
\[
K(k) = \int_0^{\frac{\pi}{2}} \frac{d\theta}{\sqrt{1 - k^2\sin^2\theta}}
\]
\[
E(k) = \int_0^{\frac{\pi}{2}} \sqrt{1 - k^2\sin^2\theta}\, d\theta
\]
And:
\[
\int_0^{\frac{\pi}{2}} \frac{\sin^2\theta}{\sqrt{1 - k^2\sin^2\theta}} d\theta = \frac{1}{k^2}\left[ K(k) - E(k) \right]
\]
Let \(k^2 = 0.0625\), \(k = 0.25\).

So,
\[
I = 0.125\left[ K(0.25) - \frac{1}{0.0625}(K(0.25) - E(0.25)) \right]
= 0.125\left[ K(0.25) - 16(K(0.25)-E(0.25)) \right]
= 0.125\left[ K(0.25) - 16K(0.25) + 16E(0.25) \right]
= 0.125\left[ -15K(0.25) + 16E(0.25) \right]
\]
\[
I = 0.125 \left( 16E(0.25) - 15K(0.25) \right)
\]

**Step 5: Final Analytical Answer**

Thus,
\[
I = 0.125 \left[ 16E(0.25) - 15K(0.25) \right]
\]

**Step 6: Numerical Approximation**

Let’s calculate the values:
- \(K(0.25) \approx 1.5962422221\)
- \(E(0.25) \approx 1.5307576369\)

So,
\[
16E(0.25) - 15K(0.25) \approx 16 \times 1.5307576369 - 15 \times 1.5962422221 = 24.49212219 - 23.9436333315 = 0.5484888585
\]
\[
I \approx 0.125 \times 0.5484888585 = 0.0685611073
\]

**Step 7: Final JSON**

```json
{"answer": "0.125\\left[16\\,E(0.25)-15\\,K(0.25)\\right]", "numerical_answer": "0.0685611073"}
```