

To solve the definite integral \(\int_{-1}^1 x^2 \cdot \sqrt[3]{x^3 + 1} \, dx\), we proceed as follows:

### Step 1: Substitution
Let \( u = x^3 + 1 \). Then, the derivative \( du/dx = 3x^2 \), so \( du = 3x^2 \, dx \), which implies \( x^2 \, dx = \frac{1}{3} du \).

### Step 2: Adjust Limits of Integration
When \( x = -1 \), \( u = (-1)^3 + 1 = 0 \). When \( x = 1 \), \( u = 1^3 + 1 = 2 \). Thus, the integral transforms to:
\[
\int_{-1}^1 x^2 \cdot \sqrt[3]{x^3 + 1} \, dx = \int_{0}^{2} \sqrt[3]{u} \cdot \frac{1}{3} du
\]

### Step 3: Evaluate the Integral
The integrand simplifies to \(\frac{1}{3} \int_{0}^{2} u^{1/3} \, du\). The antiderivative of \( u^{1/3} \) is \(\frac{3}{4} u^{4/3}\). Thus:
\[
\frac{1}{3} \int_{0}^{2} u^{1/3} \, du = \frac{1}{3} \left[ \frac{3}{4} u^{4/3} \right]_{0}^{2} = \frac{1}{4} \left[ u^{4/3} \right]_{0}^{2}
\]

### Step 4: Compute the Definite Integral
Evaluating at the bounds:
\[
\frac{1}{4} \left( 2^{4/3} - 0^{4/3} \right) = \frac{1}{4} \cdot 2^{4/3}
\]

### Step 5: Simplify the Result
Since \( 2^{4/3} = 2 \cdot 2^{1/3} \), we have:
\[
\frac{1}{4} \cdot 2 \cdot 2^{1/3} = \frac{1}{2} \cdot 2^{1/3} = \frac{\sqrt[3]{2}}{2}
\]

### Numerical Approximation
The cube root of 2 is approximately \( 1.259921049894873 \). Dividing by 2 gives \( 0.6299605249474365 \), which rounds to \( 0.6299605249 \) when rounded to 10 decimal places.

{"answer": "\\frac{\\sqrt[3]{2}}{2}", "numerical_answer": "0.6299605249"}