
To solve the definite integral \(\int_0^1 \arctan(x^2 - x + 1) \, dx\), we proceed as follows:

### Step 1: Integration by Parts
Let \( u = \arctan(x^2 - x + 1) \) and \( dv = dx \). Then:
- \( du = \frac{2x - 1}{1 + (x^2 - x + 1)^2} \, dx \)
- \( v = x \)

By integration by parts:
\[
\int \arctan(x^2 - x + 1) \, dx = x \arctan(x^2 - x + 1) - \int \frac{x(2x - 1)}{1 + (x^2 - x + 1)^2} \, dx
\]

### Step 2: Evaluate Boundary Terms
Evaluate \( x \arctan(x^2 - x + 1) \) from \( 0 \) to \( 1 \):
- At \( x = 1 \): \( 1 \cdot \arctan(1^2 - 1 + 1) = \arctan(1) = \frac{\pi}{4} \)
- At \( x = 0 \): \( 0 \cdot \arctan(0^2 - 0 + 1) = 0 \)

Thus, the boundary term is \( \frac{\pi}{4} - 0 = \frac{\pi}{4} \).

### Step 3: Simplify the Remaining Integral
The remaining integral is:
\[
\int_0^1 \frac{x(2x - 1)}{1 + (x^2 - x + 1)^2} \, dx
\]

### Step 4: Factor the Denominator
Note that \( 1 + (x^2 - x + 1)^2 = (x^2 + 1)(x^2 - 2x + 2) \). This factorization allows partial fraction decomposition.

### Step 5: Partial Fraction Decomposition
Decompose the integrand:
\[
\frac{x(2x - 1)}{(x^2 + 1)(x^2 - 2x + 2)} = \frac{-x}{x^2 + 1} + \frac{x}{x^2 - 2x + 2}
\]

### Step 6: Integrate Term by Term
Integrate each term separately:
- For \( \int \frac{-x}{x^2 + 1} \, dx \), let \( u = x^2 + 1 \), \( du = 2x \, dx \), giving \( -\frac{1}{2} \ln|x^2 + 1| \).
- For \( \int \frac{x}{x^2 - 2x + 2} \, dx \), complete the square \( x^2 - 2x + 2 = (x - 1)^2 + 1 \). Substitute \( t = x - 1 \), leading to \( \frac{1}{2} \ln|(x - 1)^2 + 1| + \arctan(x - 1) \).

### Step 7: Combine Results
Evaluating these integrals from \( 0 \) to \( 1 \) and simplifying shows the remaining integral equals \( - \ln 2 + \frac{\pi}{4} \).

### Step 8: Final Result
Subtracting this from the boundary term:
\[
\int_0^1 \arctan(x^2 - x + 1) \, dx = \frac{\pi}{4} - \left( -\ln 2 + \frac{\pi}{4} \right) = \ln 2
\]

### Numerical Approximation
The numerical value of \( \ln 2 \) is approximately \( 0.6931471806 \).

{"answer": "\(\ln 2\)", "numerical_answer": "0.6931471806"}