

To solve the definite integral \(\int_{0}^{2} H_{3}\left(\sqrt{x(2-x)}\right) \, dx\), we follow these steps:

### Step 1: Recall the third Hermite polynomial
The third Hermite polynomial is \(H_{3}(t) = 8t^{3} - 12t\). Substituting \(t = \sqrt{x(2-x)}\), the integrand becomes:
\[
H_{3}\left(\sqrt{x(2-x)}\right) = 8\left(\sqrt{x(2-x)}\right)^{3} - 12\left(\sqrt{x(2-x)}\right).
\]

### Step 2: Simplify the integrand
Note that \(x(2-x) = 1 - (x-1)^{2}\) (by completing the square). Let \(t = x - 1\), so \(x = t + 1\) and \(dx = dt\). When \(x = 0\), \(t = -1\); when \(x = 2\), \(t = 1\). Thus, \(x(2-x) = 1 - t^{2}\), and the integral transforms to:
\[
\int_{-1}^{1} \left[8(1 - t^{2})^{3/2} - 12(1 - t^{2})^{1/2}\right] dt.
\]

### Step 3: Evaluate the integrals
The integrals are symmetric around \(t = 0\), so we compute from \(0\) to \(1\) and double the result. For the first term:
\[
\int_{-1}^{1} (1 - t^{2})^{3/2} dt = 2 \int_{0}^{1} (1 - t^{2})^{3/2} dt.
\]
Using the substitution \(t = \sin\theta\) (\(dt = \cos\theta \, d\theta\)), the integral becomes:
\[
2 \int_{0}^{\pi/2} \cos^{4}\theta \, d\theta = 2 \cdot \frac{3\pi}{16} = \frac{3\pi}{8}.
\]
For the second term:
\[
\int_{-1}^{1} (1 - t^{2})^{1/2} dt = 2 \int_{0}^{1} (1 - t^{2})^{1/2} dt.
\]
Using the same substitution \(t = \sin\theta\), the integral becomes:
\[
2 \int_{0}^{\pi/2} \cos^{2}\theta \, d\theta = 2 \cdot \frac{\pi}{4} = \frac{\pi}{2}.
\]

### Step 4: Combine the results
The original integral is:
\[
8 \cdot \frac{3\pi}{8} - 12 \cdot \frac{\pi}{2} = 3\pi - 6\pi = -3\pi.
\]

### Numerical Approximation
The numerical value of \(-3\pi\) is approximately \(-9.4247779608\) (rounded to 10 decimal places).

{"answer": "$-3\\pi$", "numerical_answer": "-9.4247779608"}