We start with the integral

  I = ∫₀² H₃(√(x(2 – x))) dx.

In the physicists’ convention the Hermite polynomial H₃(x) is defined by
  H₃(x) = 8x³ – 12x.
Thus,
  H₃(√(x(2 – x))) = 8[x(2 – x)]^(3/2) – 12[x(2 – x)]^(1/2).

Substitute this into the integral:
  I = 8∫₀² [x(2 – x)]^(3/2) dx – 12∫₀² [x(2 – x)]^(1/2) dx.
We denote these integrals by
  I₁ = ∫₀² [x(2 – x)]^(3/2) dx  and  I₂ = ∫₀² [x(2 – x)]^(1/2) dx.
Then,
  I = 8 I₁ – 12 I₂.

To evaluate I₁ and I₂, we use the substitution
  x = 2 sin²θ  ⇒  dx = 4 sinθ cosθ dθ.
When x = 0, sinθ = 0 so θ = 0; when x = 2, sin²θ = 1 so θ = π/2.
Notice also that
  2 – x = 2 cos²θ,
so that
  x(2 – x) = (2 sin²θ)(2 cos²θ) = 4 sin²θ cos²θ.
Thus,
  [x(2 – x)]^(1/2) = 2 sinθ cosθ  and  [x(2 – x)]^(3/2) = (2 sinθ cosθ)³ = 8 sin³θ cos³θ.

Now we transform I₁:
  I₁ = ∫₀² [x(2 – x)]^(3/2) dx
    = ∫₀^(π/2) 8 sin³θ cos³θ · (4 sinθ cosθ dθ)
    = 32 ∫₀^(π/2) sin⁴θ cos⁴θ dθ.
Thus, the contribution from I₁ is
  8 I₁ = 8 · 32 ∫₀^(π/2) sin⁴θ cos⁴θ dθ = 256 ∫₀^(π/2) sin⁴θ cos⁴θ dθ.

Similarly, for I₂:
  I₂ = ∫₀² [x(2 – x)]^(1/2) dx
    = ∫₀^(π/2) 2 sinθ cosθ · (4 sinθ cosθ dθ)
    = 8 ∫₀^(π/2) sin²θ cos²θ dθ.
Thus, the contribution from I₂ is
  12 I₂ = 12 · 8 ∫₀^(π/2) sin²θ cos²θ dθ = 96 ∫₀^(π/2) sin²θ cos²θ dθ.

So the original integral becomes:
  I = 256 ∫₀^(π/2) sin⁴θ cos⁴θ dθ – 96 ∫₀^(π/2) sin²θ cos²θ dθ.

We now evaluate these two standard integrals.

A standard formula is:
  ∫₀^(π/2) sin^mθ cos^nθ dθ = (1/2) B((m+1)/2, (n+1)/2),
where B(a, b) is the beta function.

For the first integral, let m = 4 and n = 4:
  J₁ = ∫₀^(π/2) sin⁴θ cos⁴θ dθ = ½ B((5/2), (5/2)).
Recall that:
  B(a, b) = Γ(a)Γ(b)/Γ(a+b),
and that:
  Γ(5/2) = (3√π)/4,  Γ(5) = 24.
Thus,
  J₁ = ½ · [(Γ(5/2))²/Γ(5)] = ½ · [((3√π)/4)²/24] = ½ · [(9π/16)/24] = 9π/(768).
This can be simplified as
  J₁ = (3π/256).

For the second integral, with m = 2 and n = 2:
  J₂ = ∫₀^(π/2) sin²θ cos²θ dθ = ½ B((3/2), (3/2)).
We know:
  Γ(3/2) = (√π)/2,  Γ(3) = 2.
Thus,
  J₂ = ½ · [((√π)/2)²/2] = ½ · [(π/4)/2] = π/16.

Now plug these results back into I:
  I = 256 J₁ – 96 J₂
    = 256 · (3π/256) – 96 · (π/16)
    = 3π – (96π/16)
    = 3π – 6π
    = –3π.

Thus, the exact answer is –3π.

A numerical approximation is:
  –3π ≈ –3 × 3.141592653589793 ≈ –9.4247779608.

{"answer": "-3\\pi", "numerical_answer": "-9.4247779608"}