
To solve the definite integral \(\int\limits_0^2 x^{-1/2} I_0\left(\sqrt[4]{x(2-x)}\right)dx\), we proceed as follows:

### Step 1: Series Expansion of the Bessel Function
The modified Bessel function of the first kind \(I_0(z)\) has the series representation:
\[
I_0(z) = \sum_{n=0}^{\infty} \frac{(z^2/4)^n}{(n!)^2}
\]
Substituting \(z = \sqrt[4]{x(2-x)}\), we get \(z^2 = \sqrt{x(2-x)}\). Thus,
\[
I_0\left(\sqrt[4]{x(2-x)}\right) = \sum_{n=0}^{\infty} \frac{\left(x(2-x)\right)^{n/2}}{4^n (n!)^2}
\]

### Step 2: Interchange Sum and Integral
Assuming uniform convergence, we interchange the sum and integral:
\[
\int_0^2 x^{-1/2} I_0\left(\sqrt[4]{x(2-x)}\right) dx = \sum_{n=0}^{\infty} \frac{1}{4^n (n!)^2} \int_0^2 x^{-1/2} \left(x(2-x)\right)^{n/2} dx
\]

### Step 3: Simplify the Integrand
The integrand simplifies to:
\[
x^{-1/2} \left(x(2-x)\right)^{n/2} = x^{(n-1)/2} (2-x)^{n/2}
\]

### Step 4: Beta Function Substitution
Using the substitution \(x = 2t\) (so \(dx = 2dt\)), the integral becomes:
\[
\int_0^2 x^{(n-1)/2} (2-x)^{n/2} dx = 2^{(2n+1)/2} \int_0^1 t^{(n-1)/2} (1-t)^{n/2} dt
\]
The integral \(\int_0^1 t^a (1-t)^b dt\) is the Beta function \(B(a+1, b+1) = \frac{\Gamma(a+1)\Gamma(b+1)}{\Gamma(a+b+2)}\). Here, \(a = \frac{n-1}{2}\) and \(b = \frac{n}{2}\), so:
\[
\int_0^1 t^{(n-1)/2} (1-t)^{n/2} dt = \frac{\Gamma\left(\frac{n+1}{2}\right) \Gamma\left(\frac{n+2}{2}\right)}{\Gamma\left(n + \frac{3}{2}\right)}
\]

### Step 5: Combine Terms
Substituting back, the integral becomes:
\[
\sum_{n=0}^{\infty} \frac{\sqrt{2} \cdot 2^{-n} \Gamma\left(\frac{n+1}{2}\right) \Gamma\left(\frac{n+2}{2}\right)}{(n!)^2 \Gamma\left(n + \frac{3}{2}\right)}
\]

### Step 6: Numerical Approximation
Summing the first few terms of the series (up to \(n=3\)) gives a numerical approximation of approximately \(3.3239\).

### Final Answer
The exact answer is the series derived above, and the numerical approximation is approximately \(3.3239\).

```json
{"answer": "\\sum_{n=0}^{\\infty} \\frac{\\sqrt{2} \\cdot 2^{-n} \\Gamma\\left(\\frac{n+1}{2}\\right) \\Gamma\\left(\\frac{n+2}{2}\\right)}{(n!)^2 \\Gamma\\left(n + \\frac{3}{2}\\right)}", "numerical_answer": "3.3239"}
```