

To calculate the definite integral \(\int_{0}^{1} \arcsin(x) \arccos(x) \, dx\), we proceed as follows:

### Step 1: Use the identity \(\arcsin(x) + \arccos(x) = \frac{\pi}{2}\)
For \(x \in [-1, 1]\), \(\arccos(x) = \frac{\pi}{2} - \arcsin(x)\). Substituting this into the integrand:
\[
\arcsin(x) \arccos(x) = \arcsin(x) \left( \frac{\pi}{2} - \arcsin(x) \right) = \frac{\pi}{2} \arcsin(x) - (\arcsin(x))^2
\]
Thus, the integral becomes:
\[
\int_{0}^{1} \arcsin(x) \arccos(x) \, dx = \frac{\pi}{2} \int_{0}^{1} \arcsin(x) \, dx - \int_{0}^{1} (\arcsin(x))^2 \, dx
\]

### Step 2: Compute \(\int_{0}^{1} \arcsin(x) \, dx\)
Using integration by parts with \(u = \arcsin(x)\) and \(dv = dx\), we get \(du = \frac{1}{\sqrt{1 - x^2}} \, dx\) and \(v = x\). Thus:
\[
\int \arcsin(x) \, dx = x \arcsin(x) - \int \frac{x}{\sqrt{1 - x^2}} \, dx
\]
For the remaining integral, substitute \(t = 1 - x^2\), \(dt = -2x \, dx\), so:
\[
\int \frac{x}{\sqrt{1 - x^2}} \, dx = -\sqrt{1 - x^2} + C
\]
Combining these results:
\[
\int \arcsin(x) \, dx = x \arcsin(x) + \sqrt{1 - x^2} + C
\]
Evaluating from \(0\) to \(1\):
\[
\left[ x \arcsin(x) + \sqrt{1 - x^2} \right]_{0}^{1} = \left( 1 \cdot \frac{\pi}{2} + 0 \right) - \left( 0 + 1 \right) = \frac{\pi}{2} - 1
\]

### Step 3: Compute \(\int_{0}^{1} (\arcsin(x))^2 \, dx\)
Again, use integration by parts with \(u = (\arcsin(x))^2\) and \(dv = dx\), so \(du = \frac{2 \arcsin(x)}{\sqrt{1 - x^2}} \, dx\) and \(v = x\). Thus:
\[
\int (\arcsin(x))^2 \, dx = x (\arcsin(x))^2 - 2 \int \frac{x \arcsin(x)}{\sqrt{1 - x^2}} \, dx
\]
For the remaining integral, substitute \(t = \arcsin(x)\) (so \(x = \sin(t)\), \(dx = \cos(t) \, dt\), and \(\sqrt{1 - x^2} = \cos(t)\)):
\[
\int \frac{x \arcsin(x)}{\sqrt{1 - x^2}} \, dx = \int t \sin(t) \, dt
\]
Integrate by parts with \(u = t\) and \(dv = \sin(t) \, dt\), so \(du = dt\) and \(v = -\cos(t)\):
\[
\int t \sin(t) \, dt = -t \cos(t) + \sin(t) + C
\]
Substituting back \(t = \arcsin(x)\), \(\cos(t) = \sqrt{1 - x^2}\), and \(\sin(t) = x\):
\[
\int \frac{x \arcsin(x)}{\sqrt{1 - x^2}} \, dx = -\arcsin(x) \sqrt{1 - x^2} + x + C
\]
Thus, the original integral becomes:
\[
\int (\arcsin(x))^2 \, dx = x (\arcsin(x))^2 + 2 \arcsin(x) \sqrt{1 - x^2} - 2x + C
\]
Evaluating from \(0\) to \(1\):
\[
\left[ x (\arcsin(x))^2 + 2 \arcsin(x) \sqrt{1 - x^2} - 2x \right]_{0}^{1} = \left( 1 \cdot \left( \frac{\pi}{2} \right)^2 + 0 - 2 \cdot 1 \right) - 0 = \frac{\pi^2}{4} - 2
\]

### Step 4: Combine the results
The original integral is:
\[
\frac{\pi}{2} \left( \frac{\pi}{2} - 1 \right) - \left( \frac{\pi^2}{4} - 2 \right) = \frac{\pi^2}{4} - \frac{\pi}{2} - \frac{\pi^2}{4} + 2 = 2 - \frac{\pi}{2}
\]

### Numerical Approximation
Using \(\pi \approx 3.141592653589793\), we get:
\[
2 - \frac{\pi}{2} \approx 2 - 1.5707963267948966 = 0.4292036732051034
\]
Rounded to 10 decimal places: \(0.4292036732\).

{"answer": "2 - \\frac{\\pi}{2}", "numerical_answer": "0.4292036732"}