To evaluate the definite integral

$$
\int_0^1 \left(\frac{x^2}{2 - x^2} + \sqrt{\frac{2x}{x+1}}\right) dx,
$$

we proceed by splitting it into two parts:

$$
I = \int_0^1 \frac{x^2}{2 - x^2} dx + \int_0^1 \sqrt{\frac{2x}{x+1}} dx.
$$

---

### **First Integral:**
$$
\int_0^1 \frac{x^2}{2 - x^2} dx
$$

We simplify the integrand by expressing it as:

$$
\frac{x^2}{2 - x^2} = -1 + \frac{2}{2 - x^2}.
$$

Thus, the integral becomes:

$$
\int_0^1 \left(-1 + \frac{2}{2 - x^2}\right) dx = -\int_0^1 dx + 2 \int_0^1 \frac{1}{2 - x^2} dx.
$$

The first term is simply:

$$
-\int_0^1 dx = -1.
$$

For the second term, we use the standard integral:

$$
\int \frac{1}{a^2 - x^2} dx = \frac{1}{2a} \ln\left|\frac{a + x}{a - x}\right| + C.
$$

Here, $ a = \sqrt{2} $, so:

$$
2 \int_0^1 \frac{1}{2 - x^2} dx = 2 \cdot \left[\frac{1}{2\sqrt{2}} \ln\left(\frac{\sqrt{2} + x}{\sqrt{2} - x}\right)\right]_0^1 = \frac{1}{\sqrt{2}} \ln\left(\frac{\sqrt{2} + 1}{\sqrt{2} - 1}\right).
$$

Therefore, the first integral evaluates to:

$$
-1 + \frac{1}{\sqrt{2}} \ln\left(\frac{\sqrt{2} + 1}{\sqrt{2} - 1}\right).
$$

---

### **Second Integral:**
$$
\int_0^1 \sqrt{\frac{2x}{x+1}} dx
$$

We use the substitution:

$$
t = \sqrt{\frac{2x}{x+1}} \Rightarrow t^2 = \frac{2x}{x+1} \Rightarrow x = \frac{t^2}{2 - t^2}, \quad dx = \frac{4t}{(2 - t^2)^2} dt.
$$

The limits transform as:
- When $ x = 0 $, $ t = 0 $
- When $ x = 1 $, $ t = 1 $

So the integral becomes:

$$
\int_0^1 \sqrt{\frac{2x}{x+1}} dx = \int_0^1 t \cdot \frac{4t}{(2 - t^2)^2} dt = \int_0^1 \frac{4t^2}{(2 - t^2)^2} dt.
$$

We rewrite the integrand as:

$$
\frac{4t^2}{(2 - t^2)^2} = \frac{8}{(2 - t^2)^2} - \frac{4}{2 - t^2}.
$$

Now, integrate term by term:

- $ \int \frac{1}{2 - t^2} dt = \frac{1}{2\sqrt{2}} \ln\left(\frac{\sqrt{2} + t}{\sqrt{2} - t}\right) $
- $ \int \frac{1}{(2 - t^2)^2} dt = \frac{t}{2(2 - t^2)} + \frac{1}{4\sqrt{2}} \ln\left(\frac{\sqrt{2} + t}{\sqrt{2} - t}\right) $

Putting it all together:

$$
\int_0^1 \left(\frac{8}{(2 - t^2)^2} - \frac{4}{2 - t^2} \right) dt = \left[ \frac{4t}{2 - t^2} \right]_0^1 = \frac{4 \cdot 1}{2 - 1} = 4.
$$

But this contradicts numerical estimates.