# Calculating $\int_{-4}^4e^{|x|}\cdot\{x\}\mathsf{dx}$

Let me compute this definite integral step by step. Here, $\{x\}$ represents the fractional part of $x$, which is defined as $\{x\} = x - \lfloor x \rfloor$.

## Step 1: Break down the interval and simplify
First, I'll break down the integral based on the properties of $|x|$ and $\{x\}$.

For $|x|$:
- When $x < 0$, $|x| = -x$
- When $x \geq 0$, $|x| = x$

For $\{x\}$:
- When $x < 0$, $\{x\} = x - \lfloor x \rfloor$
- When $x \geq 0$, $\{x\} = x - \lfloor x \rfloor$

I'll split the integral at $x = 0$:
$$\int_{-4}^4e^{|x|}\cdot\{x\}\mathsf{dx} = \int_{-4}^0e^{-x}\cdot\{x\}\mathsf{dx} + \int_{0}^4e^{x}\cdot\{x\}\mathsf{dx}$$

## Step 2: Calculate the first part of the integral
For $x \in [-4,0]$, I need to analyze $\{x\}$ carefully.
- For $x \in [-4,-3]$, $\{x\} = x - (-4) = x+4$
- For $x \in [-3,-2]$, $\{x\} = x - (-3) = x+3$
- For $x \in [-2,-1]$, $\{x\} = x - (-2) = x+2$
- For $x \in [-1,0]$, $\{x\} = x - (-1) = x+1$

So I need to calculate:
$$\int_{-4}^0e^{-x}\cdot\{x\}\mathsf{dx} = \int_{-4}^{-3}e^{-x}(x+4)\mathsf{dx} + \int_{-3}^{-2}e^{-x}(x+3)\mathsf{dx} + \int_{-2}^{-1}e^{-x}(x+2)\mathsf{dx} + \int_{-1}^{0}e^{-x}(x+1)\mathsf{dx}$$

Let's calculate each integral using the formula $\int e^{-x}(ax+b)dx = -e^{-x}(ax+b) - ae^{-x} + C$:

$$\int_{-4}^{-3}e^{-x}(x+4)\mathsf{dx} = [-e^{-x}(x+4) - e^{-x}]_{-4}^{-3} = [-e^3((-3)+4) - e^3] - [-e^4((-4)+4) - e^4] = -e^3 - e^3 + e^4 = -2e^3 + e^4$$

$$\int_{-3}^{-2}e^{-x}(x+3)\mathsf{dx} = [-e^{-x}(x+3) - e^{-x}]_{-3}^{-2} = [-e^2((-2)+3) - e^2] - [-e^3((-3)+3) - e^3] = -e^2 - e^2 + e^3 = -2e^2 + e^3$$

$$\int_{-2}^{-1}e^{-x}(x+2)\mathsf{dx} = [-e^{-x}(x+2) - e^{-x}]_{-2}^{-1} = [-e^1((-1)+2) - e^1] - [-e^2((-2)+2) - e^2] = -e^1 - e^1 + e^2 = -2e^1 + e^2$$

$$\int_{-1}^{0}e^{-x}(x+1)\mathsf{dx} = [-e^{-x}(x+1) - e^{-x}]_{-1}^{0} = [-e^0((0)+1) - e^0] - [-e^1((-1)+1) - e^1] = -1 - 1 + e^1 = -2 + e^1$$

Adding these results:
$$\int_{-4}^0e^{-x}\cdot\{x\}\mathsf{dx} = (-2e^3 + e^4) + (-2e^2 + e^3) + (-2e^1 + e^2) + (-2 + e^1)$$
$$= e^4 - e^3 - e^2 - e^1 - 2$$

## Step 3: Calculate the second part of the integral
For $x \in [0,4]$, I need to analyze $\{x\}$ carefully.
- For $x \in [0,1]$, $\{x\} = x$
- For $x \in [1,2]$, $\{x\} = x-1$
- For $x \in [2,3]$, $\{x\} = x-2$
- For $x \in [3,4]$, $\{x\} = x-3$

So I need to calculate:
$$\int_{0}^4e^{x}\cdot\{x\}\mathsf{dx} = \int_{0}^{1}e^{x} \cdot x \mathsf{dx} + \int_{1}^{2}e^{x} \cdot (x-1) \mathsf{dx} + \int_{2}^{3}e^{x} \cdot (x-2) \mathsf{dx} + \int_{3}^{4}e^{x} \cdot (x-3) \mathsf{dx}$$

Let's calculate each integral using the formula $\int e^x(ax+b)dx = e^x(ax+b) - ae^x + C$:

$$\int_{0}^{1}e^{x} \cdot x \mathsf{dx} = [e^x \cdot x - e^x]_{0}^{1} = [e^1 \cdot 1 - e^1] - [e^0 \cdot 0 - e^0] = e - e + 1 = 1$$

$$\int_{1}^{2}e^{x} \cdot (x-1) \mathsf{dx} = [e^x(x-1) - e^x]_{1}^{2} = [e^2(2-1) - e^2] - [e^1(1-1) - e^1] = e^2 - e^2 - 0 + e = e$$

$$\int_{2}^{3}e^{x} \cdot (x-2) \mathsf{dx} = [e^x(x-2) - e^x]_{2}^{3} = [e^3(3-2) - e^3] - [e^2(2-2) - e^2] = e^3 - e^3 - 0 + e^2 = e^2$$

$$\int_{3}^{4}e^{x} \cdot (x-3) \mathsf{dx} = [e^x(x-3) - e^x]_{3}^{4} = [e^4(4-3) - e^4] - [e^3(3-3) - e^3] = e^4 - e^4 - 0 + e^3 = e^3$$

Adding these results:
$$\int_{0}^4e^{x}\cdot\{x\}\mathsf{dx} = 1 + e + e^2 + e^3$$

## Step 4: Combine the results
Now I'll add both parts of the integral:
$$\int_{-4}^4e^{|x|}\cdot\{x\}\mathsf{dx} = (e^4 - e^3 - e^2 - e^1 - 2) + (1 + e + e^2 + e^3)$$
$$= e^4 - e^3 - e^2 - e^1 - 2 + 1 + e^1 + e^2 + e^3$$
$$= e^4 - 1$$

## Step 5: Numerical approximation
$e^4 = 54.59815003$, so $e^4 - 1 = 53.59815003$

Rounded to 10 decimal places: $53.5981500332$

{"answer": "e^4 - 1", "numerical_answer": "53.5981500332"}