<think>
Okay, let's tackle this integral step by step. The integral given is from 0 to 7 of the function ∛(√(x² + 1) + x) minus ∛(√(x² + 1) - x) dx. Hmm, that looks a bit complicated with the cube roots and square roots. I need to find an analytical solution first.

Let me start by simplifying the integrand. Maybe there's a substitution that can make this easier. Let's denote the two cube root terms as A and B, where A = ∛(√(x² + 1) + x) and B = ∛(√(x² + 1) - x). The integrand is A - B. If I can find a relationship between A and B, that might help.

Let me compute A³ and B³ to see if there's a pattern. 

A³ = √(x² + 1) + x  
B³ = √(x² + 1) - x  

If I add A³ and B³, I get 2√(x² + 1). If I subtract them, I get 2x. But how does that help with A - B?

Alternatively, maybe if I set t = A - B, then perhaps t³ can be expressed in terms of A and B. Let's try expanding (A - B)³:

t³ = A³ - B³ - 3AB(A - B)  
We know A³ - B³ = (√(x² +1) + x) - (√(x² +1) - x) = 2x  
So t³ = 2x - 3AB t  
But AB is ∛(A³ B³). Let's compute A³ * B³:

A³)(B³) = (√(x² +1) + x)(√(x² +1) - x) = (x² +1) - x² = 1  
So AB = ∛1 = 1. Therefore, AB = 1.  

So substituting back into the equation for t³:  
t³ = 2x - 3(1)t  
Which simplifies to t³ + 3t - 2x = 0.  

Wait, but our integrand is t = A - B, and we have a differential equation involving t and x. Maybe we can express x in terms of t and then integrate. Let's see.

From t³ + 3t - 2x = 0, we can solve for x:  
x = (t³ + 3t)/2  

Now, if we can express dx in terms of dt, we can change the variable of integration from x to t. Let's compute dx/dt:

dx/dt = (3t² + 3)/2 = (3/2)(t² + 1)  

So, dx = (3/2)(t² + 1) dt  

Now, we need to adjust the limits of integration. When x = 0, let's t?  

At x = 0:  
t = A - B = ∛(√(0 +1) +0) - ∛(√(0 +1) -0) = ∛1 - ∛1 = 0. So when x=0, t=0.  

When x =7, we need to compute t. Let's compute t when x=7:  
t³ + 3t - 14 =0. Hmm, solving this cubic equation. Let's try possible integer roots. Testing t=2: 8 +6 -14=0. Yes! So t=2 is a root. Therefore, when x=7, t=2.  

So the integral from x=0 to x=7 becomes the integral from t=0 to t=2 of t * dx. Since the original integrand is t, and dx is (3/2)(t² +1) dt. Therefore, the integral becomes:

∫₀² t * (3/2)(t² +1) dt = (3/2) ∫₀² (t³ + t) dt  

Integrate term by term:  
∫ t³ dt = t⁴/4  
∫ t dt = t²/2  

So the integral is (3/2)[ (t⁴/4 + t²/2) ] from 0 to 2.  

Calculating at t=2:  
(16/4 + 4/2) = 4 + 2 =6  
At t=0, it's 0.  

So the integral is (3/2)(6 -0) = (3/2)*6 =9.  

Wait, so the exact answer is 9? Let me check that again.  

Yes, the substitution seems correct. Let me verify the steps again.  

1. Let t = A - B.  
2. Then t³ = 2x - 3t.  
3. Solving for x gives x = (t³ +3t)/2.  
4. Then dx/dt = (3t² +3)/2.  
5. The integral becomes ∫ t * (3/2)(t² +1) dt from t=0 to t=2.  
6. Which simplifies to (3/2) ∫ (t³ + t) dt from 0 to 2.  
7. The integral of t³ is t⁴/4, and t is t²/2.  
8. Evaluated at 2: (16/4 +4/2)=4+2=6.  
9. Multiply by 3/2: 6*(3/2)=9.  

Yes, that's correct. So the exact value of the integral is 9. The numerical approximation is 9.0000000000.  

But wait, let me check if there's any mistake in substitution. For example, when x=7, t=2. Let's confirm that.  

At x=7, t³ +3t =14. Plugging t=2: 8 +6=14. Correct. So the upper limit is indeed 2.  

Therefore, the integral is exactly 9. The numerical approximation is 9.0, which when rounded to 10 decimal places is 9.0000000000.  

I think that's the solution. Let me just recap to make sure I didn't skip any steps. The key insight was to set t as the integrand, then find a relation between t and x, perform substitution, and then the integral simplifies nicely. The substitution worked out perfectly with the limits, leading to a straightforward calculation. So the answer is 9.
</think>

{"answer": "9", "numerical_answer": "9.0000000000"}