To solve the definite integral 

\[
\int_{420}^{1672} \frac{\sqrt{\ln(2023 - x)}}{\sqrt{\ln(2023 - x)} + \sqrt{\ln(x - 69)}} \, dx,
\]

we can follow these steps:

### Step 1: Symmetry and Substitution

Let’s denote the integrand as 

\[
f(x) = \frac{\sqrt{\ln(2023 - x)}}{\sqrt{\ln(2023 - x)} + \sqrt{\ln(x - 69)}}}.
\]

We observe that the limits of integration \( a = 420 \) and \( b = 1672 \) are symmetric around the point \( c = \frac{a + b}{2} = \frac{420 + 1672}{2} = 1046 \). 

Let’s perform the substitution \( x = 1046 + t \), which shifts the integral to be symmetric around \( t = 0 \):

\[
\int_{-626}^{626} f(1046 + t) \, dt.
\]

However, it's more insightful to consider the substitution \( x = 2023 - (x - 69) \), but let's instead use the substitution \( y = 2023 + 69 - x = 2092 - x \). 

When \( x = 420 \), \( y = 1672 \), and when \( x = 1672 \), \( y = 420 \). The differential \( dx = -dy \), so the integral becomes:

\[
\int_{y=1672}^{420} \frac{\sqrt{\ln(y - 69)}}{\sqrt{\ln(y - 69)} + \sqrt{\ln(2023 - y)}} (-dy) = \int_{420}^{1672} \frac{\sqrt{\ln(y - 69)}}{\sqrt{\ln(y - 69)} + \sqrt{\ln(2023 - y)}} \, dy.
\]

Now, notice that the original integral \( I \) is:

\[
I = \int_{420}^{1672} \frac{\sqrt{\ln(2023 - x)}}{\sqrt{\ln(2023 - x)} + \sqrt{\ln(x - 69)}} \, dx,
\]

and the transformed integral is:

\[
I = \int_{420}^{1672} \frac{\sqrt{\ln(x - 69)}}{\sqrt{\ln(x - 69)} + \sqrt{\ln(2023 - x)}} \, dx.
\]

Adding these two expressions for \( I \):

\[
2I = \int_{420}^{1672} \left( \frac{\sqrt{\ln(2023 - x)} + \sqrt{\ln(x - 69)}}{\sqrt{\ln(2023 - x)} + \sqrt{\ln(x - 69)}} \right) dx = \int_{420}^{1672} 1 \, dx = 1672 - 420 = 1252.
\]

Thus, 

\[
I = \frac{1252}{2} = 626.
\]

### Step 2: Numerical Verification

The exact value of the integral is \( 626 \). The numerical approximation is simply:

\[
626.0000000000.
\]

### Final Answer

```json
{"answer": "626", "numerical_answer": "626.0000000000"}
```