Let's proceed step by step:

We are asked to evaluate:
\[
I = \int_0^\infty x^{2-1} e^{-1.0x^2} H_2(1.0x) \, dx
\]
Let's interpret this clearly. Here, \( x^{2-1} = x \), and \( H_2(y) \) is the 2nd Hermite polynomial. The "1.0" is just a scaling parameter, so \( H_2(1.0x) \).

Recall:
\[
H_2(x) = 4x^2 - 2
\]
Thus,
\[
H_2(1.0x) = 4(1.0x)^2 - 2 = 4x^2 - 2
\]

The integral becomes:
\[
I = \int_0^\infty x \, e^{-x^2} (4x^2 - 2) dx
\]
Expand:
\[
I = \int_0^\infty x \, e^{-x^2} \cdot 4x^2 \, dx - \int_0^\infty x \, e^{-x^2} \cdot 2 \, dx
\]
\[
= 4 \int_0^\infty x^3 e^{-x^2} dx - 2 \int_0^\infty x e^{-x^2} dx
\]
Now, let's compute both terms.

**First term:**
\[
\int_0^\infty x^3 e^{-x^2} dx
\]

Substitute \( u = x^2 \implies du = 2x dx \implies x dx = \frac{du}{2} \):

When \( x = 0, u = 0 \). As \( x \rightarrow \infty, u \rightarrow \infty \).

\( x^3 e^{-x^2} dx = x^2 \cdot x e^{-x^2} dx = x^2 e^{-x^2} \cdot x dx \).

Let’s write:
\[
x^3 e^{-x^2} dx = x^2 \cdot x e^{-x^2} dx = x^2 e^{-x^2} \cdot x dx = x^2 e^{-x^2} \cdot \frac{du}{2}
\]

But, \( x^2 = u \):
\[
\int_0^\infty x^3 e^{-x^2} dx = \int_{u=0}^\infty u e^{-u} \cdot \frac{du}{2}
= \frac{1}{2} \int_0^\infty u e^{-u} du
\]

But \( \int_0^\infty u e^{-u} du = \Gamma(2) = 1! = 1 \).
So:
\[
\int_0^\infty x^3 e^{-x^2} dx = \frac{1}{2} \times 1 = \frac{1}{2}
\]

**Second term:**
\[
\int_0^\infty x e^{-x^2} dx
\]

Let’s use the same substitution, \( u = x^2 \implies du = 2x dx \implies x dx = \frac{du}{2} \).
So,
\[
\int_0^\infty x e^{-x^2} dx = \int_{u=0}^\infty e^{-u} \frac{du}{2} = \frac{1}{2} \int_0^\infty e^{-u} du = \frac{1}{2} [ -e^{-u}]_0^{\infty} = \frac{1}{2}(0 + 1) = \frac{1}{2}
\]

Putting everything together:
\[
I = 4 \cdot \frac{1}{2} - 2 \cdot \frac{1}{2} = 2 - 1 = 1
\]

**Numerical approximation:**
\( 1.0000000000 \)

**Final answer in required JSON format:**
```json
{"answer": "1", "numerical_answer": "1.0000000000"}
```