### Step 1: Substitution
Let’s consider the substitution:
\[ u = \log(\log x) \]

First, compute the derivative of \( u \) with respect to \( x \):
\[ \frac{du}{dx} = \frac{d}{dx} \left( \log(\log x) \right) = \frac{1}{\log x} \cdot \frac{1}{x} = \frac{1}{x \log x} \]

Thus, the differential \( du \) is:
\[ du = \frac{1}{x \log x} dx \]
\[ \implies x \log x \, du = dx \]

### Step 2: Rewrite the Integral
The original integral is:
\[ \int_{e}^{e^e} \frac{\log x \cdot \log(\log x)}{x} \, dx \]

Notice that:
\[ \frac{\log x \cdot \log(\log x)}{x} \, dx = \log(\log x) \cdot \left( \frac{\log x}{x} dx \right) \]

But from the substitution, we have \( dx = x \log x \, du \), so:
\[ \frac{\log x}{x} dx = \frac{\log x}{x} \cdot x \log x \, du = \log^2 x \, du \]

This seems a bit convoluted. Let’s try a different substitution.

### Step 3: Alternative Substitution
Let’s set:
\[ t = \log x \]
Then:
\[ \frac{dt}{dx} = \frac{1}{x} \implies dt = \frac{1}{x} dx \]

Now, rewrite the integral in terms of \( t \):
\[ \int_{e}^{e^e} \frac{\log x \cdot \log(\log x)}{x} \, dx = \int_{x=e}^{x=e^e} \log x \cdot \log(\log x) \cdot \frac{1}{x} \, dx \]
\[ = \int_{t=1}^{t=e} t \cdot \log t \, dt \]

Now, the integral simplifies to:
\[ \int_{1}^{e} t \log t \, dt \]

### Step 4: Integrate by Parts
To evaluate \( \int t \log t \, dt \), we use integration by parts:
\[ \int u \, dv = uv - \int v \, du \]

Let:
\[ u = \log t \implies du = \frac{1}{t} dt \]
\[ dv = t \, dt \implies v = \frac{t^2}{2} \]

Then:
\[ \int t \log t \, dt = \frac{t^2}{2} \log t - \int \frac{t^2}{2} \cdot \frac{1}{t} \, dt \]
\[ = \frac{t^2}{2} \log t - \frac{1}{2} \int t \, dt \]
\[ = \frac{t^2}{2} \log t - \frac{1}{2} \cdot \frac{t^2}{2} + C \]
\[ = \frac{t^2}{2} \log t - \frac{t^2}{4} + C \]
\[ = \frac{t^2}{4} (2 \log t - 1) + C \]

### Step 5: Evaluate the Definite Integral
Now, evaluate from \( t = 1 \) to \( t = e \):
\[ \left. \frac{t^2}{4} (2 \log t - 1) \right|_{1}^{e} \]
\[ = \frac{e^2}{4} (2 \log e - 1) - \frac{1}{4} (2 \log 1 - 1) \]
\[ = \frac{e^2}{4} (2 \cdot 1 - 1) - \frac{1}{4} (0 - 1) \]
\[ = \frac{e^2}{4} (1) + \frac{1}{4} \]
\[ = \frac{e^2}{4} + \frac{1}{4} \]
\[ = \frac{e^2 + 1}{4} \]

### Step 6: Numerical Approximation
Compute the numerical value of \( \frac{e^2 + 1}{4} \):
\[ e^2 \approx 7.3890560989 \]
\[ e^2 + 1 \approx 8.3890560989 \]
\[ \frac{e^2 + 1}{4} \approx 2.0972640247 \]

### Final Answer
The exact answer is \( \frac{e^2 + 1}{4} \), and the numerical approximation is approximately 2.0972640247.

```json
{"answer": "\\frac{e^2 + 1}{4}", "numerical_answer": "2.0972640247"}
```