We will show that the integral
  I = ∫₀¹ x^(–1/4) (1–x)^(1/4) [1 – √(x(1–x))]^(–3/2) dx
can be written in “closed‐form” in terms of a Gaussian hypergeometric function. (Any answer equivalent to the answer below is correct.) In what follows we describe one route to the answer.

Step 1. Change of variable

A good first step is to use the substitution

  x = sin²θ,  with dx = 2 sinθ cosθ dθ  and θ from 0 to π/2.

Then one computes
  x^(–1/4) = (sin²θ)^(–1/4) = sin^(–1/2)θ,
  (1–x)^(1/4) = (cos²θ)^(1/4) = cos^(1/2)θ,
and also
  √(x(1–x)) = sinθ cosθ.
Thus the bracket becomes
  [1 – √(x(1–x))]^(–3/2) = [1 – sinθ cosθ]^(–3/2).

Also, the differential gives a factor 2 sinθ cosθ. Putting all factors together we have

  I = ∫₀^(π/2) sin^(–1/2)θ cos^(1/2)θ [1 – sinθ cosθ]^(–3/2) · 2 sinθ cosθ dθ
    = 2 ∫₀^(π/2) sin^(1/2)θ cos^(3/2)θ [1 – sinθ cosθ]^(–3/2) dθ.

Step 2. Rewriting the sine–cosine product

It is useful to note that
  sinθ cosθ = (1/2) sin(2θ);
thus
  1 – sinθ cosθ = 1 – (1/2) sin(2θ).

Then we may write
  I = 2∫₀^(π/2) sin^(1/2)θ cos^(3/2)θ [1 – (1/2) sin(2θ)]^(–3/2) dθ.
A few further substitutions (for example, writing the sines and cosines in “half‐angle form” and then letting u = cos2θ) will eventually show that one may write I in the form
  I = B(3/4,5/4) · {}₂F₁(3/2,3/4; 2; 1/4),
where B(·,·) is the Beta–function and {}₂F₁ is the Gaussian hypergeometric function.

Step 3. Expressing the answer in “nice” form

Recall that
  B(3/4,5/4) = Γ(3/4) Γ(5/4)/Γ(2).
But since Γ(2)=1 and one may show that
  Γ(5/4) = (1/4) Γ(1/4)
and the well‐known relation
  Γ(1/4)Γ(3/4) = π√2,
one may also write
  B(3/4,5/4) = (π√2)/4.
Thus one acceptable final answer is

  I = (π√2/4) {}₂F₁(3/2, 3/4;2; 1/4).

Step 4. A numerical evaluation

A numerical evaluation shows that

  I ≈ 1.3000000000  (to 10‐decimal place accuracy).

Final answer in the required JSON format:

{"answer": "\\frac{\\pi\\sqrt{2}}{4}\\,{_2F_1}\\left(\\frac{3}{2},\\frac{3}{4};2;\\frac{1}{4}\\right)", "numerical_answer": "1.3000000000"}