We start with
  I = ∫₀∞ [tanh(x)/eˣ] dx.

Step 1. Rewrite tanh(x):
  tanh(x) = 1 – (2/(e^(2x)+1)).
Thus,
  I = ∫₀∞ [e^(–x) – 2e^(–x)/(e^(2x)+1)] dx
    = ∫₀∞ e^(–x) dx – 2J,
where
  J = ∫₀∞ e^(–x)/(e^(2x)+1) dx.

Step 2. The first integral is simple:
  ∫₀∞ e^(–x) dx = [–e^(–x)]₀∞ = 1.

Step 3. Evaluate J by substitution. Let u = e^x so that:
  e^(–x) = 1/u  and  dx = du/u,
and when x = 0, u = 1; when x → ∞, u → ∞.
Then,
  J = ∫₁∞ [1/u] / (1+u²) · (du/u)
    = ∫₁∞ 1/(u² (1+u²)) du.

Step 4. Decompose the integrand:
Notice that
  1/(u²(1+u²)) = 1/u² – 1/(1+u²).
This is verified by writing:
  1/u² – 1/(1+u²) = [(1+u²) – u²] / (u²(1+u²)) = 1/(u²(1+u²)).

Thus,
  J = ∫₁∞ [1/u² – 1/(1+u²)] du
    = ∫₁∞ 1/u² du – ∫₁∞ 1/(1+u²) du.

Step 5. Compute the individual integrals:
(i) ∫₁∞ 1/u² du = [–1/u]₁∞ = (0 – (–1)) = 1.
(ii) ∫₁∞ 1/(1+u²) du = [arctan(u)]₁∞ = (π/2 – arctan(1)) = π/2 – π/4 = π/4.

Thus,
  J = 1 – π/4.

Step 6. Substitute back into I:
  I = 1 – 2J = 1 – 2(1 – π/4) = 1 – 2 + (π/2) = (π/2) – 1.

Step 7. Numerical approximation:
  π/2 ≈ 1.5707963268, so
  I ≈ 1.5707963268 – 1 = 0.5707963268 (rounded to 10 decimal places).

Final answer in JSON format:
{"answer": "\\frac{\\pi}{2} - 1", "numerical_answer": "0.5707963268"}