We wish to evaluate

  I = ∫₀² x^(1/2) (2 – x)^(–1/2) cosh(√(x(2 – x))) dx.

Step 1. Make the substitution x = 1 + cos θ.
 • Then 2 – x = 1 – cos θ.
 • Also x(2 – x) = (1 + cos θ)(1 – cos θ) = 1 – cos²θ = sin²θ, so that √(x(2 – x)) = sin θ.
 • The differential is dx = – sin θ dθ.
 • When x = 0: 1 + cos θ = 0 ⟹ cos θ = –1 ⟹ θ = π.
 • When x = 2: 1 + cos θ = 2 ⟹ cos θ = 1 ⟹ θ = 0.
 
Thus,
  I = ∫ₜ₌₋π^0 [√(1 + cos θ) (1/√(1 – cos θ)) cosh(sin θ)] (– sin θ dθ).

Flipping the limits gives

  I = ∫₀ᴨ [√(1+cos θ)/√(1–cos θ)] cosh(sin θ) sin θ dθ.

Step 2. Simplify the integrand.
Recall the half-angle formulas:
  1 + cos θ = 2 cos²(θ/2),  1 – cos θ = 2 sin²(θ/2).
Thus,
  √(1+cos θ)/√(1–cos θ) = (√(2) cos(θ/2))/(√(2) sin(θ/2)) = cot(θ/2).
Also, note that sin θ = 2 sin(θ/2) cos(θ/2). Therefore, the product becomes

  cot(θ/2) sin θ = [cos(θ/2)/sin(θ/2)] · [2 sin(θ/2) cos(θ/2)] = 2 cos²(θ/2).

So the integral simplifies to

  I = ∫₀ᴨ 2 cos²(θ/2) cosh(sin θ) dθ.

Step 3. Change the variable.
Let u = θ/2, so that θ = 2u and dθ = 2 du.
When θ = 0, u = 0;  when θ = π, u = π/2.
Also, sin θ = sin(2u) = 2 sin u cos u.
Then

  I = ∫₀^(π/2) 2 cos²(u) cosh(2 sin u cos u) · (2 du)
     = 4 ∫₀^(π/2) cos²(u) cosh(2 sin u cos u) du.
Since 2 sin u cos u = sin 2u, we rewrite the integrand as

  I = 4 ∫₀^(π/2) cos²(u) cosh(sin 2u) du.

Step 4. Use the cosine double‐angle formula.
Write cos²(u) = (1 + cos 2u)/2 so that

  I = 4 ∫₀^(π/2) (1+cos2u)/2 · cosh(sin2u) du
     = 2 ∫₀^(π/2) [1+cos2u] cosh(sin2u) du.

Now, change variable again: let t = 2u ⟹ dt = 2 du, so that du = dt/2.
When u = 0, t = 0; when u = π/2, t = π. Then

  I = 2 ∫₀^(π) [1 + cos t] cosh(sin t) · (dt/2)
     = ∫₀^(π) [1+cos t] cosh(sin t) dt.

Step 5. Split the integral.
Write I as

  I = ∫₀^(π) cosh(sin t) dt + ∫₀^(π) cos t cosh(sin t) dt.
In the second integral, use the substitution u = sin t so that du = cos t dt. The limits become u(0)=0 and u(π)=0. Hence the second integral vanishes:

  ∫₀^(π) cos t cosh(sin t) dt = ∫₍₀₎^(0) cosh(u) du = 0.
Thus, we obtain

  I = ∫₀^(π) cosh(sin t) dt.

Step 6. Recognize a standard result.
There is a standard identity that for any real a
  ∫₀^(π) cosh(a sin t) dt = π I₀(a),
when a = 1 we see that

  I = ∫₀^(π) cosh(sin t) dt = π I₀(1),
where I₀(1) is the modified Bessel function of order zero evaluated at 1.

Step 7. Write the exact answer and its numerical approximation.
Thus, the exact answer is

  I = π I₀(1).

A numerical evaluation gives I₀(1) ≈ 1.266065877752, and hence

  I ≈ π × 1.266065877752 ≈ 3.9760261053.

Finally, we output the answer in the required JSON format.

{"answer": "$\\pi I_0(1)$", "numerical_answer": "3.9760261053"}