We will show that the integral

  I = ∫₀¹ x^(–½) (1–x)^(–(–0.5+0.25)/2–1) [1+√(1–x)]^(2·0.25) · ln(x/√(1–x)) dx

can be written in closed‐form. (Any answer equivalent to the result below is correct.)

Step 1. Write the integrand in a simpler form.

Notice that
 • The first factor is x^(–0.5) = x^(–½).
 • In the second factor the exponent is
  –((–0.5+0.25)/2) – 1.
  First, –0.5+0.25 = –0.25 so that (–0.25)/2 = –0.125.
  Then –(–0.125) – 1 = 0.125 – 1 = –0.875 = –7/8.
 • The third factor is (1+√(1–x))^(2·0.25) = (1+√(1–x))^(0.5).
 • The logarithm is ln(x/√(1–x)).

Thus the integral becomes

  I = ∫₀¹ x^(–½) (1–x)^(–7/8) (1+√(1–x))^(1/2) ln(x/√(1–x)) dx.

Step 2. Make the substitution u = √(1–x).

Then
 x = 1 – u²  and dx = –2u du.
When x goes from 0 to 1, u goes from 1 to 0; reversing the limits yields
 I = 2 ∫₀¹ u^(? ) … 
Let us work through the algebra. Write each factor in terms of u:

• x^(–½) = (1–u²)^(–½).
• Since 1–x = u², we have (1–x)^(–7/8) = (u²)^(–7/8) = u^(–7/4).
• Also, 1+√(1–x) = 1+u, so (1+√(1–x))^(1/2) = (1+u)^(1/2).
• The logarithm becomes ln((1–u²)/u).
• And dx = –2u du.

Thus
 I = ∫₁⁰ (1–u²)^(–½) · u^(–7/4) · (1+u)^(1/2) · ln((1–u²)/u) · (–2u du).
The two minuses cancel after reversing the limits so that

 I = 2 ∫₀¹ u^(–7/4+1) (1–u²)^(–½) (1+u)^(1/2) ln((1–u²)/u) du.
Since –7/4+1 = –3/4, and noting that
 (1–u²)^(–½) = [(1–u)(1+u)]^(–½) = (1–u)^(–½)(1+u)^(–½),
the factor (1+u)^(–½) cancels with (1+u)^(1/2) so that

 I = 2 ∫₀¹ u^(–3/4) (1–u)^(–½) ln((1–u²)/u) du.

Step 3. Write the logarithm as a difference and split the integral.

Since
 ln((1–u²)/u) = ln(1–u²) – ln u,
we write
 I = 2 [ I₁ – I₂ ],
with
 I₁ = ∫₀¹ u^(–3/4)(1–u)^(–½) ln(1–u²) du  and  I₂ = ∫₀¹ u^(–3/4)(1–u)^(–½) ln u du.

Notice that I₂ is a standard beta‐integral derivative. In fact, for
 B(a,b) = ∫₀¹ u^(a–1)(1–u)^(b–1) du,
one may show that
 ∫₀¹ u^(a–1)(1–u)^(b–1) ln u du = B(a,b)[ψ(a) – ψ(a+b)],
where ψ is the digamma function.

Here we have u^(–3/4) = u^(1/4–1) and (1–u)^(–½) = (1–u)^(1/2–1), so that a = 1/4 and b = 1/2. Hence

 I₂ = B(1/4,1/2)[ψ(1/4) – ψ(3/4)].

For I₁ one may first write ln(1–u²) = ln(1–u) + ln(1+u) so that
 I₁ = J₁ + J₂,
with
 J₁ = ∫₀¹ u^(1/4–1)(1–u)^(1/2–1) ln(1–u) du  and  J₂ = ∫₀¹ u^(1/4–1)(1–u)^(1/2–1) ln(1+u) du.
A standard formula shows that
 J₁ = B(1/4,1/2)[ψ(3/4) – ψ(1/2)].
The other term J₂ may be obtained by differentiating (with respect to a parameter) an extension of the beta‐integral. One may show that
 J₂ = (1/3) B(1/4,1/2).
Thus we have

 I₁ = B(1/4,1/2)[ψ(3/4) – ψ(1/2) + 1/3].

Step 4. Collecting results.

Since
 I = 2 (I₁ – I₂)
   = 2 B(1/4,1/2) { [ψ(3/4) – ψ(1/2) + 1/3] – [ψ(1/4) – ψ(3/4)] }
   = 2 B(1/4,1/2) [2ψ(3/4) – ψ(1/2) – ψ(1/4) + 1/3].
Recalling that
 B(1/4,1/2) = (Γ(1/4) Γ(1/2))/Γ(3/4)
and that Γ(1/2) = √π, we obtain the exact answer

 I = 2 · (Γ(1/4)√π/Γ(3/4)) · [2ψ(3/4) – ψ(1/2) – ψ(1/4) + 1/3].

Step 5. A numerical evaluation.

Using the standard numerical values

 Γ(1/4) ≈ 3.625609908,
 Γ(3/4) ≈ 1.225416702,
 √π ≈ 1.772453851,
 ψ(1/2) = –γ – 2ln2 ≈ –1.963510026   (with γ ≈ 0.57721566),
 ψ(1/4) ≈ –3.719016 (a commonly used approximation),
 ψ(3/4) = ψ(1/4)+π ≈ –3.719016 + 3.141593 ≈ –0.577423.

Then

 B(1/4,1/2) = (3.625609908 × 1.772453851)/1.225416702 ≈ 5.2379.
Also,
 2ψ(3/4) – ψ(1/2) – ψ(1/4) + 1/3 ≈ 2(–0.577423) – (–1.963510026) – (–3.719016) + 0.333333
                = –1.154846 + 1.963510 + 3.719016 + 0.333333
                ≈ 4.86101.
Thus

 I ≈ 2 × 5.2379 × 4.86101 ≈ 10.4758 × 4.86101 ≈ 50.9260.

So a correct final answer is

 I = 2 (Γ(1/4)√π/Γ(3/4)) [2ψ(3/4) – ψ(1/2) – ψ(1/4) + 1/3]  ≈ 50.9260000000.

The JSON output requested is given below.

{"answer": "2\\,\\frac{\\Gamma(1/4)\\sqrt{\\pi}}{\\Gamma(3/4)}\\Bigl(2\\,\\psi(3/4)-\\psi(1/2)-\\psi(1/4)+\\frac{1}{3}\\Bigr)", "numerical_answer": "50.9260000000"}