<think>
Okay, so I need to compute the definite integral from 0 to 1 of (1/x) * arccos(x) * arcsin²(x) dx. Hmm, that looks a bit complicated. Let me start by recalling some integration techniques that might help here. The integrand has arccos, arcsin, and a 1/x term. Maybe substitution or integration by parts?

First, let me note that arccos(x) and arcsin(x) are related. Since arccos(x) = π/2 - arcsin(x), maybe I can express everything in terms of arcsin(x) to simplify. Let me try that substitution. Let’s set t = arcsin(x). Then, x = sin(t), and dx = cos(t) dt. When x=0, t=0, and when x=1, t=π/2. So the integral becomes:

∫ from 0 to π/2 of [ (1/sin(t)) * (π/2 - t) * t² ] * cos(t) dt.

Simplify the integrand. The 1/sin(t) times cos(t) is cot(t). So the integral is ∫ (π/2 - t) * t² * cot(t) dt from 0 to π/2. Hmm, that still looks tricky. Maybe expanding the product (π/2 - t) * t² gives π/2 t² - t³. So split the integral into two parts:

π/2 ∫ t² cot(t) dt - ∫ t³ cot(t) dt, both from 0 to π/2.

Now, I need to compute these integrals involving t^n cot(t). I remember that integrals of t^n cot(t) can be related to series expansions or perhaps using integration by parts. Let me think about integration by parts for each integral.

Starting with the first integral: ∫ t² cot(t) dt. Let’s set u = t², dv = cot(t) dt. Then du = 2t dt, and v = ln(sin(t)). So integration by parts gives:

uv - ∫ v du = t² ln(sin(t)) - 2 ∫ t ln(sin(t)) dt.

But now the integral becomes more complicated. The second term is ∫ t ln(sin(t)) dt, which might not be straightforward. Maybe another approach is needed. Alternatively, perhaps expanding cot(t) as a series?

Recall that cot(t) can be expressed as a series. For |t| < π, cot(t) = 1/t - 2 ∑_{n=1}^∞ (ζ(2n)/π^{2n}) t^{2n -1}, but I'm not sure if that's helpful here. Alternatively, using the expansion cot(t) = ∑_{k=0}^∞ (-1)^k 2^{2k} B_{2k} t^{2k-1}/(2k)!), but that might complicate things further.

Alternatively, maybe express sin(t) in terms of its Taylor series. Let me try that. Since ln(sin(t)) can be expressed as a series. Wait, but integrating t^n ln(sin(t)) might not be easy. Maybe another substitution.

Alternatively, consider the integral ∫ t^n cot(t) dt. Let me check if there's a known formula for this. I recall that integrals involving t^n and cot(t) can sometimes be expressed in terms of the Riemann zeta function or other special functions, but I'm not sure. Let me check for n=2 and n=3.

Alternatively, perhaps using the integral representation of the zeta function. Wait, maybe integrating term by term. Let me recall that cot(t) can be written as the sum from k=0 to infinity of [ (2k)! B_{2k} (2t)^{2k-1} } / ( (2^{2k} - 1)(k!)^2 ) ) ] for |t| < π. But this seems complicated.

Alternatively, maybe using the Fourier series for ln(sin(t)). Since ln(sin(t)) = -ln(2) - ∑_{k=1}^∞ (cos(2kt))/k, valid for 0 < t < π. Then, for the integral ∫ t ln(sin(t)) dt, substituting the series gives:

- ln(2) ∫ t dt - ∑_{k=1}^∞ (1/k) ∫ t cos(2kt) dt.

Integrating term by term. The first integral is - (ln(2)/2) t². The second term involves integrating t cos(2kt) dt. Integration by parts: let u = t, dv = cos(2kt) dt. Then du = dt, v = (1/(2k)) sin(2kt). So uv - ∫ v du = (t/(2k)) sin(2kt) - ∫ (1/(2k)) sin(2kt) dt. The integral becomes (t/(2k)) sin(2kt) + (1/(4k²)) cos(2kt). Evaluated from 0 to π/2.

At t=π/2: sin(2k*(π/2)) = sin(kπ) = 0. cos(2k*(π/2)) = cos(kπ) = (-1)^k. At t=0: sin(0) = 0, cos(0) = 1. So the integral from 0 to π/2 of t cos(2kt) dt is [0 + (1/(4k²)) (-1)^k] - [0 + (1/(4k²)) (1)] = ( (-1)^k - 1 )/(4k²).

Therefore, the integral ∫ t ln(sin(t)) dt from 0 to π/2 is:

- (ln(2)/2)( (π/2)^2 ) - ∑_{k=1}^∞ (1/k) [ ( (-1)^k - 1 )/(4k²) ) ]

Simplify this expression. Let's compute each part:

First term: - (ln(2)/2)( π² /4 ) = - (π² ln 2)/8.

Second term: - (1/4) ∑_{k=1}^∞ [ ( (-1)^k - 1 ) / k^3 ]

Note that ( (-1)^k - 1 ) is -2 when k is odd, and 0 when k is even. So the sum becomes:

- (1/4) * ∑_{m=1}^∞ [ (-2) / (2m -1)^3 ] where m is 1,2,... (since k is odd, k=2m-1)

So that's (1/4) * 2 ∑_{m=1}^∞ 1/(2m -1)^3 = (1/2) ∑_{m=1}^∞ 1/(2m -1)^3.

But ∑_{m=1}^∞ 1/(2m -1)^3 = ∑_{n=1}^∞ 1/n^3 - ∑_{n=1}^∞ 1/(2n)^3 = (1 - 1/8) ζ(3) = (7/8) ζ(3). Wait, no. Wait, ζ(3) is the sum over all n, so sum_{n odd} 1/n^3 = ζ(3) - sum_{n even} 1/n^3 = ζ(3) - 1/8 ζ(3) = (7/8) ζ(3). Therefore, the second term is (1/2) * (7/8) ζ(3) = 7/16 ζ(3).

Wait, but the original expression was - (1/4) * [ sum over k odd of (-2)/k^3 ] = - (1/4) * (-2) * sum_{k odd} 1/k^3 = (1/2) sum_{k odd} 1/k^3 = (1/2)(7/8 ζ(3)) = 7/16 ζ(3). But since the original term was subtracted, the entire second term is - (1/4) * [ ... ] which becomes +7/16 ζ(3). Wait, let me check again.

Wait, the integral ∫ t ln(sin t) dt from 0 to π/2 is:

- (π² ln 2)/8 - (1/4) ∑_{k=1}^∞ [ ( (-1)^k -1 ) / k^3 ]

But ( (-1)^k -1 ) / k^3 = [ (-1)^k -1 ] / k^3. For even k, (-1)^k =1, so term is 0. For odd k, (-1)^k = -1, so term is (-1 -1)/k^3 = -2/k^3. So the sum becomes sum over odd k of (-2)/k^3. So:

- (1/4) * sum_{k odd} (-2)/k^3 = - (1/4)*(-2) sum_{k odd} 1/k^3 = (1/2) sum_{k odd} 1/k^3.

As before, sum_{k odd} 1/k^3 = (1 - 1/8) ζ(3) = 7/8 ζ(3). Therefore, the second term is (1/2)(7/8 ζ(3)) = 7/16 ζ(3). Therefore, the integral ∫ t ln(sin t) dt from 0 to π/2 is:

- (π² ln 2)/8 + 7 ζ(3)/16.

Wait, but the original expression was:

- (π² ln 2)/8 - (1/4) sum [...] which became - (π² ln 2)/8 + 7 ζ(3)/16.

So that's the value of ∫ t ln(sin t) dt from 0 to π/2. Therefore, going back to the first integral:

∫ t² cot(t) dt = t² ln(sin t) - 2 ∫ t ln(sin t) dt. Evaluated from 0 to π/2.

At t=π/2, sin(t)=1, so ln(sin t)=0. At t=0, t² ln(sin t) approaches 0 (since t² goes to 0 and ln(sin t) ~ ln t, but t² ln t approaches 0). Therefore, the boundary term is 0 - 0 = 0. So the integral becomes -2 times the integral of t ln(sin t) dt, which is:

-2 [ - (π² ln 2)/8 + 7 ζ(3)/16 ] = 2*(π² ln 2)/8 - 2*(7 ζ(3)/16 ) = (π² ln 2)/4 - 7 ζ(3)/8.

So the first integral, ∫ t² cot(t) dt from 0 to π/2 is (π² ln 2)/4 - 7 ζ(3)/8.

Now, moving to the second integral: ∫ t³ cot(t) dt from 0 to π/2. Let's use integration by parts again. Let u = t³, dv = cot(t) dt. Then du = 3t² dt, v = ln(sin t). So integration by parts gives:

uv - ∫ v du = t³ ln(sin t) - 3 ∫ t² ln(sin t) dt. Evaluated from 0 to π/2.

Again, at the limits, t³ ln(sin t) is 0 at both ends. So the integral becomes -3 ∫ t² ln(sin t) dt from 0 to π/2. But we need to compute ∫ t² ln(sin t) dt. Hmm, this seems recursive. Let's see if we can find this integral.

Wait, earlier we found ∫ t ln(sin t) dt. Maybe we can use a similar approach for ∫ t² ln(sin t) dt. Let me try expanding ln(sin t) as a Fourier series again.

So, ln(sin t) = -ln 2 - ∑_{k=1}^∞ (cos(2kt))/k. Then, ∫ t² ln(sin t) dt = -ln 2 ∫ t² dt - ∑_{k=1}^∞ (1/k) ∫ t² cos(2kt) dt.

First term: -ln 2 * (t³/3) evaluated from 0 to π/2 = -ln 2 * ( (π/2)^3 /3 ) = - (π³ ln 2)/24.

Second term: - ∑_{k=1}^∞ (1/k) ∫ t² cos(2kt) dt. Let's compute ∫ t² cos(2kt) dt. Integration by parts. Let u = t², dv = cos(2kt) dt. Then du = 2t dt, v = (1/(2k)) sin(2kt). So:

uv - ∫ v du = (t²/(2k)) sin(2kt) - (1/k) ∫ t sin(2kt) dt.

Now, compute ∫ t sin(2kt) dt. Let u = t, dv = sin(2kt) dt. Then du = dt, v = -1/(2k) cos(2kt). So:

- (1/(2k)) t cos(2kt) + (1/(2k)) ∫ cos(2kt) dt = - (t/(2k)) cos(2kt) + (1/(4k²)) sin(2kt).

Putting it all together:

∫ t² cos(2kt) dt = (t²/(2k)) sin(2kt) - (1/k)[ - (t/(2k)) cos(2kt) + (1/(4k²)) sin(2kt) ] + C

Simplify:

= (t²/(2k)) sin(2kt) + (t/(2k²)) cos(2kt) - (1/(4k³)) sin(2kt) + C.

Now evaluate from 0 to π/2:

At t=π/2:

sin(2k*(π/2)) = sin(kπ) = 0.

cos(2k*(π/2)) = cos(kπ) = (-1)^k.

sin(2k*(π/2)) = 0.

So the first term: 0.

Second term: (π/2)/(2k²) * (-1)^k.

Third term: -1/(4k³) * 0 = 0.

At t=0:

All terms are 0.

Therefore, the integral from 0 to π/2 of t² cos(2kt) dt is [ (π/(4k²)) (-1)^k ] - 0 = (π (-1)^k )/(4k²).

Therefore, the second term becomes:

- ∑_{k=1}^∞ (1/k) * [ π (-1)^k / (4k²) ) ] = π/4 ∑_{k=1}^∞ (-1)^k / k^3.

So the entire integral ∫ t² ln(sin t) dt from 0 to π/2 is:

- (π³ ln 2)/24 + π/4 ∑_{k=1}^∞ (-1)^k /k^3.

But ∑_{k=1}^∞ (-1)^k /k^3 = - (3/4) ζ(3). Wait, is that correct? Wait, the Dirichlet eta function η(s) = ∑_{k=1}^∞ (-1)^{k+1}/k^s = (1 - 2^{1-s}) ζ(s). For s=3, η(3) = ∑_{k=1}^∞ (-1)^{k+1}/k^3 = (1 - 2^{-2}) ζ(3) = (3/4) ζ(3). Therefore, ∑_{k=1}^∞ (-1)^k /k^3 = - η(3) = -3/4 ζ(3).

Therefore, the sum term is π/4 * (-3/4 ζ(3)) = - 3π ζ(3)/16.

So the integral ∫ t² ln(sin t) dt from 0 to π/2 is:

- (π³ ln 2)/24 - 3π ζ(3)/16.

Therefore, going back to the second integral ∫ t³ cot(t) dt from 0 to π/2, which was -3 times this integral:

-3 [ - (π³ ln 2)/24 - 3π ζ(3)/16 ] = 3*(π³ ln 2)/24 + 9π ζ(3)/16 = (π³ ln 2)/8 + 9π ζ(3)/16.

So putting it all together, the original integral was:

π/2 * [ (π² ln 2)/4 - 7 ζ(3)/8 ] - [ (π³ ln 2)/8 + 9π ζ(3)/16 ].

Let's compute each term:

First term: π/2 * (π² ln 2 /4) = π³ ln 2 /8.

Second term: π/2 * (-7 ζ(3)/8) = -7π ζ(3)/16.

Third term: - (π³ ln 2)/8.

Fourth term: -9π ζ(3)/16.

So combining:

π³ ln 2 /8 -7π ζ(3)/16 - π³ ln 2 /8 -9π ζ(3)/16.

The first and third terms cancel out (π³ ln2/8 - π³ ln2/8 = 0), and the remaining terms:

-7π ζ(3)/16 -9π ζ(3)/16 = -16π ζ(3)/16 = -π ζ(3).

So the integral ∫_0^1 (1/x) arccos(x) arcsin²(x) dx equals -π ζ(3). Wait, but ζ(3) is a positive number (approximately 1.2020569...), so the integral is negative? But the integrand is (1/x) arccos(x) arcsin²(x). Let's check the integrand's sign. For x in (0,1), arccos(x) is positive, arcsin(x) is positive, and 1/x is positive. So the integrand is positive, but the result is negative? That can't be. There must be a mistake in the sign somewhere.

Wait, this suggests I made an error in the calculation. Let me trace back.

Original substitution: t = arcsin(x), so x = sin(t), dx = cos(t) dt. The integral becomes:

∫ from 0 to π/2 [ (1/sin(t)) * (π/2 - t) * t² ] * cos(t) dt.

Which is ∫ (π/2 - t) t² cot(t) dt. So expanding, it's π/2 ∫ t² cot(t) dt - ∫ t³ cot(t) dt.

Then, when we computed ∫ t² cot(t) dt, we got (π² ln2)/4 -7 ζ(3)/8.

Then ∫ t³ cot(t) dt was (π³ ln2)/8 +9π ζ(3)/16.

But when we substituted back into the original expression:

π/2 * [ (π² ln2)/4 -7 ζ(3)/8 ] - [ (π³ ln2)/8 +9π ζ(3)/16 ]

Let me compute each term again:

π/2 * (π² ln2 /4) = (π^3 ln2)/8.

π/2 * (-7 ζ(3)/8) = -7 π ζ(3)/16.

Then subtract the second integral: - (π³ ln2)/8 -9π ζ(3)/16.

So total:

(π³ ln2)/8 -7π ζ(3)/16 - π³ ln2/8 -9π ζ(3)/16 = 0 - (7+9)π ζ(3)/16 = -16π ζ(3)/16 = -π ζ(3).

But the integral of a positive function can't be negative. So there's a mistake in the sign. Let me check the substitution step.

Original integral: ∫ (1/x) arccos(x) arcsin²(x) dx from 0 to1.

Substitution: x = sin(t), so dx = cos(t) dt. Then 1/x = 1/sin(t), arccos(x) = arccos(sin(t)) = π/2 - t (since arccos(sin t) = π/2 - t when t in [0, π/2]). So the integrand becomes:

(1/sin(t)) * (π/2 - t) * t²) * cos(t) dt = (π/2 - t) t² cot(t) dt.

So the integral is ∫ (π/2 - t) t² cot(t) dt from 0 to π/2. So expanding, it's π/2 ∫ t² cot(t) dt - ∫ t³ cot(t) dt.

But when we computed these integrals, we ended up with -π ζ(3). But since the integrand is positive, the result should be positive. Therefore, there must be a sign error in the calculation.

Let me check the integration by parts steps. For the first integral, ∫ t² cot(t) dt:

We set u = t², dv = cot(t) dt. Then du = 2t dt, v = ln(sin t). So uv - ∫ v du = t² ln(sin t) - 2 ∫ t ln(sin t) dt. Evaluated from 0 to π/2, the boundary term is 0, so the integral is -2 ∫ t ln(sin t) dt. Then we computed ∫ t ln(sin t) dt as - (π² ln2)/8 +7 ζ(3)/16. Therefore, -2 times that is (π² ln2)/4 -7 ζ(3)/8. That seems correct.

For the second integral, ∫ t³ cot(t) dt:

Set u = t³, dv = cot(t) dt. Then du = 3t² dt, v = ln(sin t). So uv - ∫ v du = t³ ln(sin t) -3 ∫ t² ln(sin t) dt. Evaluated from 0 to π/2, boundary term is 0, so integral is -3 ∫ t² ln(sin t) dt. Then we computed ∫ t² ln(sin t) dt as - (π³ ln2)/24 -3π ζ(3)/16. Therefore, -3 times that is 3*(π³ ln2)/24 +9π ζ(3)/16 = (π³ ln2)/8 +9π ζ(3)/16. That seems correct.

Then the original expression is π/2*(first integral) - (second integral):

π/2*( (π² ln2)/4 -7 ζ(3)/8 ) - ( (π³ ln2)/8 +9π ζ(3)/16 )

Compute π/2*(π² ln2/4) = π³ ln2/8.

π/2*(-7 ζ(3)/8) = -7π ζ(3)/16.

Subtract the second integral: - (π³ ln2/8 +9π ζ(3)/16 ) = -π³ ln2/8 -9π ζ(3)/16.

Adding all terms:

π³ ln2/8 -7π ζ(3)/16 -π³ ln2/8 -9π ζ(3)/16 = 0 -16π ζ(3)/16 = -π ζ(3).

But the integral should be positive. So where is the mistake? The substitution step must have a sign error. Let me check the substitution again.

Wait, when x = sin(t), then arccos(x) = arccos(sin(t)). For t in [0, π/2], arccos(sin(t)) = π/2 - t. That's correct. So the integrand is (π/2 - t) * t² * cot(t). cot(t) is cos(t)/sin(t), which is positive in (0, π/2). So the integrand is positive. Therefore, the integral should be positive. But our result is negative. So there's a mistake in the calculation.

Wait, when we computed ∫ t ln(sin t) dt, we got - (π² ln2)/8 +7 ζ(3)/16. Then multiplied by -2 gives (π² ln2)/4 -7 ζ(3)/8. Then the first integral is π/2 times that: π/2*(π² ln2/4 -7 ζ(3)/8) = π³ ln2/8 -7π ζ(3)/16.

Then the second integral is ∫ t³ cot(t) dt = (π³ ln2)/8 +9π ζ(3)/16.

So the original integral is π³ ln2/8 -7π ζ(3)/16 - (π³ ln2/8 +9π ζ(3)/16) = π³ ln2/8 -7π ζ(3)/16 -π³ ln2/8 -9π ζ(3)/16 = (-7π ζ(3)/16 -9π ζ(3)/16) = -16π ζ(3)/16 = -π ζ(3).

But this is negative. Contradicts the positive integrand. Therefore, there must be a mistake in the sign somewhere. Let me check the Fourier series expansion of ln(sin t).

Wait, ln(sin t) = -ln 2 - ∑_{k=1}^∞ cos(2kt)/k. So when we integrated t ln(sin t) dt, we had:

∫ t ln(sin t) dt = -ln2 ∫ t dt - ∑_{k=1}^∞ (1/k) ∫ t cos(2kt) dt.

Which became - (ln2/2)(π²/4) - ∑_{k=1}^∞ (1/k) [ ( (-1)^k -1 )/(4k²) ]

But when we evaluated ∫ t cos(2kt) dt from 0 to π/2, we got ( (-1)^k -1 )/(4k²). But wait, let me recheck that integral.

Earlier, when integrating t cos(2kt) dt from 0 to π/2, we had:

uv - ∫ v du = (t/(2k)) sin(2kt) - ∫ (1/(2k)) sin(2kt) dt.

The integral of sin(2kt) is -cos(2kt)/(2k). So:

= (t/(2k)) sin(2kt) + (1/(4k²)) cos(2kt) evaluated from 0 to π/2.

At t=π/2: sin(kπ)=0, cos(kπ)=(-1)^k.

At t=0: sin(0)=0, cos(0)=1.

So the integral is [0 + (1/(4k²)) (-1)^k] - [0 + (1/(4k²)) *1] = [ (-1)^k -1 ]/(4k²).

Therefore, the integral of t cos(2kt) dt from 0 to π/2 is [ (-1)^k -1 ]/(4k²). So the sum becomes:

- ∑_{k=1}^∞ (1/k) * [ ( (-1)^k -1 )/(4k²) ) ] = - (1/4) ∑_{k=1}^∞ [ ( (-1)^k -1 ) /k^3 ].

As before, this becomes (1/2) sum_{k odd} 1/k^3 = 7/16 ζ(3). So the integral ∫ t ln(sin t) dt is - (π² ln2)/8 +7 ζ(3)/16. Then multiplying by -2 gives (π² ln2)/4 -7 ζ(3)/8. So far, correct.

Then the first integral is π/2 times that: π/2*(π² ln2/4 -7 ζ(3)/8) = π³ ln2/8 -7π ζ(3)/16.

Then the second integral ∫ t³ cot(t) dt = -3 ∫ t² ln(sin t) dt. We computed ∫ t² ln(sin t) dt as - (π³ ln2)/24 -3π ζ(3)/16. Therefore, -3 times that is (π³ ln2)/8 +9π ζ(3)/16.

So the original integral is:

π³ ln2/8 -7π ζ(3)/16 - π³ ln2/8 -9π ζ(3)/16 = -16π ζ(3)/16 = -π ζ(3).

But this is negative. Contradiction. Therefore, there must be a mistake in the sign during substitution.

Wait, when we did the substitution x = sin(t), dx = cos(t) dt. The original integral is from x=0 to x=1, which becomes t=0 to t=π/2. The integrand is (1/x) arccos(x) arcsin²(x) dx. So substituting, we have:

(1/sin(t)) * (π/2 - t) * t² * cos(t) dt.

But 1/sin(t) * cos(t) is cot(t). So the integrand is (π/2 - t) t² cot(t) dt. Which is correct.

But cot(t) is cos(t)/sin(t), which is positive in (0, π/2). So the integrand is positive. Therefore, the integral should be positive. But our result is negative. So there's a mistake in the sign somewhere.

Wait, perhaps the substitution step is correct, but the evaluation of the integrals has a sign error. Let me check the integral of t ln(sin t) dt again.

We had:

∫ t ln(sin t) dt = - (π² ln2)/8 +7 ζ(3)/16.

But when we multiplied by -2, we get (π² ln2)/4 -7 ζ(3)/8. Then π/2 times that is π³ ln2/8 -7π ζ(3)/16.

Then the second integral is -3 times ∫ t² ln(sin t) dt. Which was computed as -3*(-π³ ln2/24 -3π ζ(3)/16) = π³ ln2/8 +9π ζ(3)/16.

So the original integral is π³ ln2/8 -7π ζ(3)/16 - π³ ln2/8 -9π ζ(3)/16 = -π ζ(3).

But this is negative. Therefore, the mistake must be in the sign of the integral of t ln(sin t) dt. Let me recheck that.

When we expanded ln(sin t) as -ln2 - ∑_{k=1}^∞ cos(2kt)/k, then ∫ t ln(sin t) dt = -ln2 ∫ t dt - ∑_{k=1}^∞ (1/k) ∫ t cos(2kt) dt.

The first term is -ln2*(t²/2) evaluated from 0 to π/2, which is -ln2*(π²/8).

The second term is - ∑_{k=1}^∞ (1/k) * [ ( (-1)^k -1 )/(4k²) ].

Which is - (1/4) ∑_{k=1}^∞ [ ( (-1)^k -1 ) /k^3 ].

As before, this sum is over k odd, and equals (1/2) sum_{k odd} 1/k^3 = 7/16 ζ(3).

So the integral is - (π² ln2)/8 +7 ζ(3)/16.

But wait, the integral of t ln(sin t) dt from 0 to π/2 is negative? Let's check with a numerical example. For example, at t=π/4, ln(sin t) is negative, and t is positive, so the product is negative. So the integral from 0 to π/2 of a negative function would be negative. But according to the calculation, it's - (π² ln2)/8 +7 ζ(3)/16. Let's compute this numerically.

Compute - (π² ln2)/8 +7 ζ(3)/16.

π² ≈ 9.8696, ln2 ≈ 0.6931, so π² ln2 ≈ 9.8696 *0.6931 ≈ 6.832. Divided by 8: ≈ 0.854.

7 ζ(3)/16: ζ(3) ≈ 1.2020569, so 7*1.2020569 ≈ 8.4144. Divided by 16: ≈ 0.5259.

So total: -0.854 +0.5259 ≈ -0.3281. So the integral ∫ t ln(sin t) dt from 0 to π/2 is approximately -0.3281. Which is negative, which makes sense because the integrand is negative. Then multiplying by -2 gives approximately 0.6562. Then π/2 times that is approximately 1.030.

The second integral ∫ t³ cot(t) dt was computed as (π³ ln2)/8 +9π ζ(3)/16. Let's compute that:

π³ ≈ 31.006, ln2 ≈0.6931, so π³ ln2 ≈31.006*0.6931≈21.5. Divided by 8: ≈2.6875.

9π ζ(3)/16: 9*3.1416*1.2020569≈9*3.1416*1.202≈34.202. Divided by 16≈2.1376.

So total: 2.6875 +2.1376≈4.8251.

Then the original integral is 1.030 -4.8251≈-3.7951. But ζ(3)≈1.202, so -π ζ(3)≈-3.773. Which is close to the approximate calculation. But the integral should be positive. So there's a contradiction.

Therefore, there must be a mistake in the substitution step. Let me check again.

Wait, the original integral is ∫ (1/x) arccos(x) arcsin²(x) dx from 0 to1.

But when we substitute x = sin(t), then 1/x = 1/sin(t), arccos(x) = π/2 - t, arcsin(x) = t. So arcsin²(x) = t². So the integrand becomes (1/sin(t)) * (π/2 - t) * t² * cos(t) dt.

Which is (π/2 - t) t² cot(t) dt. So the integral is ∫ (π/2 - t) t² cot(t) dt from 0 to π/2.

But cot(t) is cos(t)/sin(t), which is positive. The term (π/2 - t) is positive for t in [0, π/2). So the integrand is positive. Therefore, the integral must be positive. But our result is negative. Therefore, there must be a mistake in the sign during integration by parts.

Wait, when we did the first integration by parts for ∫ t² cot(t) dt, we set u = t², dv = cot(t) dt. Then du = 2t dt, v = ln(sin t). So uv - ∫ v du = t² ln(sin t) - 2 ∫ t ln(sin t) dt. Evaluated from 0 to π/2, the boundary term is 0. So the integral is -2 ∫ t ln(sin t) dt. But ∫ t ln(sin t) dt is negative, so -2 times a negative is positive. Then the first integral is positive. Similarly, the second integral ∫ t³ cot(t) dt is -3 ∫ t² ln(sin t) dt. Since ∫ t² ln(sin t) dt is negative, -3 times that is positive. So both integrals are positive. Then the original integral is π/2*(positive) - (positive). But according to our calculation, it's negative, which is impossible. Therefore, there must be a mistake in the sign when expanding the original integral.

Wait, the original integral is π/2 ∫ t² cot(t) dt - ∫ t³ cot(t) dt. Both integrals are positive. So π/2*(positive) - (positive). Depending on the values, it could be positive or negative. But according to our calculation, it's negative, which contradicts the integrand being positive. Therefore, the mistake must be in the calculation of the integrals.

Alternatively, perhaps the integral ∫ t² ln(sin t) dt is computed incorrectly. Let me recheck that.

We had:

∫ t² ln(sin t) dt = - (π³ ln2)/24 -3π ζ(3)/16.

But let's compute this numerically. For example, take t=π/2. The integral from 0 to π/2 of t² ln(sin t) dt. Let's approximate it numerically. Let's use numerical integration.

But since I can't compute it here, let's see. If the integral is negative, then multiplying by -3 gives a positive term, which when subtracted from the first term could give a negative result. But the original integral should be positive. Therefore, the mistake must be in the sign of the integral ∫ t² ln(sin t) dt.

Wait, when we computed ∫ t² ln(sin t) dt, we used the expansion ln(sin t) = -ln2 - ∑_{k=1}^∞ cos(2kt)/k. Then:

∫ t² ln(sin t) dt = -ln2 ∫ t² dt - ∑_{k=1}^∞ (1/k) ∫ t² cos(2kt) dt.

The first term is -ln2*(π³/24). The second term is - ∑_{k=1}^∞ (1/k) * [ π (-1)^k / (4k²) ] = - π/4 ∑_{k=1}^∞ (-1)^k /k^3.

But ∑_{k=1}^∞ (-1)^k /k^3 = -η(3) = - (1 - 2^{1-3}) ζ(3) = - (3/4) ζ(3). So the second term is - π/4 * (-3/4 ζ(3)) = 3π ζ(3)/16.

Therefore, the integral ∫ t² ln(sin t) dt is - (π³ ln2)/24 +3π ζ(3)/16.

Wait, previously I had - (π³ ln2)/24 -3π ζ(3)/16. That's where the mistake was! The sum ∑_{k=1}^∞ (-1)^k /k^3 is -η(3) = -3/4 ζ(3). So the second term is - π/4 * (-3/4 ζ(3)) = +3π ζ(3)/16. Therefore, the integral is - (π³ ln2)/24 +3π ζ(3)/16. Not minus. So the correct expression is:

∫ t² ln(sin t) dt from 0 to π/2 = - (π³ ln2)/24 +3π ζ(3)/16.

Therefore, the second integral ∫ t³ cot(t) dt is -3 times that:

-3*(- (π³ ln2)/24 +3π ζ(3)/16 ) = 3*(π³ ln2)/24 -9π ζ(3)/16 = (π³ ln2)/8 -9π ζ(3)/16.

Now, substituting back into the original expression:

π/2 * [ (π² ln2)/4 -7 ζ(3)/8 ] - [ (π³ ln2)/8 -9π ζ(3)/16 ].

Compute each term:

First term: π/2*(π² ln2/4) = π³ ln2/8.

Second term: π/2*(-7 ζ(3)/8) = -7π ζ(3)/16.

Third term: - (π³ ln2)/8.

Fourth term: +9π ζ(3)/16.

So combining:

π³ ln2/8 -7π ζ(3)/16 -π³ ln2/8 +9π ζ(3)/16 = (π³ ln2/8 -π³ ln2/8) + (-7π ζ(3)/16 +9π ζ(3)/16) = 0 +2π ζ(3)/16 = π ζ(3)/8.

Wait, that's different. So the integral equals π ζ(3)/8. Which is positive, as expected. So the mistake was in the sign of the integral ∫ t² ln(sin t) dt. Previously, I had a minus instead of a plus.

Therefore, the correct result is π ζ(3)/8. Let me verify this.

So, after correcting the sign in the integral ∫ t² ln(sin t) dt, the second integral becomes (π³ ln2)/8 -9π ζ(3)/16. Then the original integral is:

π/2*(first integral) - second integral = π³ ln2/8 -7π ζ(3)/16 - (π³ ln2/8 -9π ζ(3)/16) = π³ ln2/8 -7π ζ(3)/16 -π³ ln2/8 +9π ζ(3)/16 = (0) + (2π ζ(3)/16) = π ζ(3)/8.

Yes, that makes sense. So the integral evaluates to π ζ(3)/8. Which is approximately π * 1.2020569 /8 ≈ 3.14159265 *1.2020569 /8 ≈ 3.773 /8 ≈ 0.4716. Let me compute this numerically:

ζ(3) ≈ 1.2020569031595942853997381615114499907649862923405.

π ≈ 3.1415926535897932384626433832795028841971693993751.

So π * ζ(3) ≈ 3.141592653589793 *1.202056903159594 ≈ 3.774330738.

Divided by 8: 3.774330738 /8 ≈0.47179134225.

So the numerical value is approximately 0.47179134225.

Therefore, the exact answer is π ζ(3)/8, and the numerical approximation is approximately 0.4717913423.

But wait, let me check with numerical integration to confirm. Let's approximate the original integral numerically.

The integral is ∫₀¹ (1/x) arccos(x) arcsin²(x) dx.

Let me approximate this using substitution x = sin(t), which gives ∫₀^{π/2} (π/2 - t) t² cot(t) dt.

Using numerical integration method, let's approximate this integral.

But since I can't compute it here, but given that the analytical result is π ζ(3)/8 ≈0.4717913423, and the integrand is positive, this seems plausible.

Therefore, the final answer is π ζ(3)/8, and the numerical approximation is approximately 0.4717913423.
</think>

{"answer": "\\frac{\\pi \\zeta(3)}{8}", "numerical_answer": "0.4717913423"}