Let's denote the definite integral as
\[
I = \int_{0}^{2} x^{1/2} (2-x)^{1/2} \cos\left( \sqrt{x(2-x)} \right) dx.
\]

**Step 1: Symmetry and substitution**

Let \( x = 2\sin^2\theta \) for \( \theta \in [0, \pi/2] \).

Then,
\[
dx = 4\sin\theta \cos\theta \, d\theta = 2\sin(2\theta) \, d\theta
\]
\[
x^{1/2} = \sqrt{2}\sin\theta
\]
\[
2-x = 2-2\sin^2\theta = 2\cos^2\theta
\implies (2-x)^{1/2} = \sqrt{2}\cos\theta
\]
\[
x(2-x) = 2\sin^2\theta \cdot 2\cos^2\theta = 4\sin^2\theta\cos^2\theta = (\sin 2\theta)^2
\]
\[
\sqrt{x(2-x)} = \sin 2\theta
\]

Plug everything into the integral:

\[
I = \int_{\theta=0}^{\theta=\pi/2} (\sqrt{2}\sin\theta)(\sqrt{2}\cos\theta) \cos(\sin 2\theta) \cdot 2\sin(2\theta)d\theta
\]

\[
= \int_{0}^{\pi/2} 2\sin\theta\cos\theta \cdot \cos(\sin 2\theta) \cdot 2\sin(2\theta)d\theta
\]

Recall: \( \sin\theta\cos\theta = \frac{1}{2}\sin 2\theta \):
\[
2\sin\theta\cos\theta = \sin 2\theta
\]

\[
I = \int_{0}^{\pi/2} \sin 2\theta \cdot \cos(\sin 2\theta) \cdot 2\sin(2\theta)d\theta
= 2 \int_{0}^{\pi/2} \sin^2 2\theta \cos(\sin 2\theta)d\theta
\]

**Step 2: Substitute \( u = \sin 2\theta \), \( du = 2\cos 2\theta d\theta \)**

When \(\theta = 0\), \(u=0\)

When \(\theta = \pi/2\), \(u = \sin \pi = 0\)

But over the interval \([0, \pi/2]\), \(u\) goes from 0 to 1 (at \(\theta = \pi/4\)), then back to 0 (at \(\theta = \pi/2\)). Therefore, to express as a single definite integral, split interval at \(\pi/4\):

- When \( \theta = 0 \), \(u = 0\)
- When \( \theta = \pi/4 \), \(u = \sin(\pi/2) = 1 \)
- When \( \theta = \pi/2 \), \(u = \sin(\pi) = 0 \)

\( d\theta = \frac{du}{2\cos 2\theta} \), but for \(\cos 2\theta = \sqrt{1-u^2}\) for \(\theta\) in \([0, \pi/4]\), negative in \((\pi/4,\pi/2]\).

Compute for \([0, \pi/4]\): as \(u\) increases from 0 to 1,

\[
2 \int_{\theta=0}^{\theta=\pi/2} \sin^2 2\theta \cos(\sin 2\theta) d\theta
= 2 \left(\int_{\theta=0}^{\theta=\pi/4} + \int_{\theta=\pi/4}^{\theta=\pi/2}\right) \sin^2 2\theta \cos(\sin 2\theta) d\theta
\]

But \(\cos 2\theta\) is positive in \(0 \leq \theta < \pi/4\), negative in \(\pi/4 < \theta \leq \pi/2\).

So,

For \([0, \pi/4]\):

Let \(u = \sin 2\theta\), \( d\theta = du / (2\cos 2\theta) = du/(2 \sqrt{1-u^2}) \):

\[
2 \int_{\theta=0}^{\theta=\pi/4} \sin^2 2\theta \cos(\sin 2\theta) d\theta
= 2 \int_{u=0}^{u=1} u^2 \cos(u) \frac{du}{2\sqrt{1-u^2}}
= \int_{u=0}^{u=1} \frac{u^2 \cos u}{\sqrt{1-u^2}} du
\]

Now for \([\pi/4, \pi/2]\), as \(\theta\) increases from \(\pi/4\) to \(\pi/2\), \(u\) decreases from 1 to 0.

So \( du = -|du| \). On this interval, \(\cos 2\theta = -\sqrt{1-u^2}\):

Therefore,

\[
2 \int_{\theta=\pi/4}^{\theta=\pi/2} \sin^2 2\theta \cos(\sin 2\theta) d\theta
= 2 \int_{u=1}^{u=0} u^2 \cos u \frac{du}{-2 \sqrt{1-u^2}}
= -\int_{u=1}^{u=0} \frac{u^2 \cos u}{\sqrt{1-u^2}} du = \int_{u=0}^{u=1} \frac{u^2 \cos u}{\sqrt{1-u^2}} du
\]

Therefore,

\[
I = 2 \int_{u=0}^{u=1} \frac{u^2 \cos u}{\sqrt{1-u^2}} du
\]

**Step 3: Analytical solution**

Let’s focus on evaluating:

\[
I = 2 \int_{0}^{1} \frac{u^2 \cos u}{\sqrt{1-u^2}} du
\]

Let’s use substitution:

Let’s recall that \( \int_0^1 \frac{u^2 \cos(a u)}{\sqrt{1-u^2}} du = \frac{\pi}{4} [ J_0(a) + J_2(a) ] \), where \( J_n \) are Bessel functions of the first kind. (This is a standard integral from tables.)

In our case, the argument of cosine is just \(u\).

So,

\[
I = 2 \int_{0}^{1} \frac{u^2 \cos(u)}{\sqrt{1-u^2}} du = 2 \cdot \frac{\pi}{4} ( J_0(1) + J_2(1) ) = \frac{\pi}{2} ( J_0(1) + J_2(1) )
\]

**Step 4: Numerical value**

Let’s recall:

- \( J_0(1) \approx 0.7651976866 \)
- \( J_2(1) \approx 0.1149034849 \)
- So \( J_0(1) + J_2(1) \approx 0.8801011715 \)
- \( \frac{\pi}{2} \approx 1.5707963268 \)

Finally,
\[
I \approx 1.5707963268 \times 0.8801011715 \approx 1.3824485275
\]

**Final JSON Output**
```json
{"answer": "\\frac{\\pi}{2}\\left[J_0(1) + J_2(1)\\right]", "numerical_answer": "1.3824485275"}
```