Let’s compute the definite integral:
\[
I = \int_{0}^{1} \arccos(x)\arctan(x) \, dx
\]

### Step 1: Analytical Solution

Let’s see if we can express this integral in terms of known constants or elementary functions.

Let:
\[
I = \int_{0}^{1} \arccos(x)\arctan(x) \, dx
\]

#### Approach: Integration by Parts

Let’s use integration by parts:
Let
- \( u = \arccos(x) \implies du = -\frac{1}{\sqrt{1-x^2}}dx \)
- \( dv = \arctan(x) dx \implies v = \int \arctan(x) dx \)

We need \( \int \arctan(x) dx \):
\[
\int \arctan(x) dx = x\arctan(x) - \frac{1}{2} \ln(1+x^2) + C
\]

Applying integration by parts:
\[
I = uv \bigg|_{0}^{1} - \int_{0}^{1} v \, du
\]

So:
\[
I = \left[ \arccos(x) \left( x\arctan(x) - \frac{1}{2} \ln(1+x^2) \right) \right]_{0}^{1}
+ \int_{0}^{1} \left( x\arctan(x) - \frac{1}{2} \ln(1+x^2) \right) \frac{1}{\sqrt{1-x^2}} dx
\]

But recall that \( du = -1 / \sqrt{1-x^2}\, dx \), so actually the integral sign flips:
\[
I = \left[ \arccos(x) \left( x\arctan(x) - \frac{1}{2} \ln(1+x^2) \right) \right]_{0}^{1}
+ \int_{0}^{1} \frac{x\arctan(x) - \frac{1}{2} \ln(1+x^2)}{\sqrt{1-x^2}} dx
\]

##### Let’s compute the boundary terms

At \( x=1 \):
- \( \arccos(1) = 0 \)
- \( \arctan(1) = \frac{\pi}{4} \)
- \( \ln(1+1^2) = \ln(2) \)

So, first term at \( x=1 \) is:
\[
0 \cdot (1\cdot \frac{\pi}{4} - \frac{1}{2}\ln 2) = 0
\]

At \( x=0 \):
- \( \arccos(0) = \frac{\pi}{2} \)
- \( \arctan(0) = 0 \)
- \( \ln(1+0^2) = \ln(1) = 0 \)

Thus, first term at \( x=0 \) is:
\[
\frac{\pi}{2} (0 - 0) = 0
\]

So the first bracket gives zero.

Thus,
\[
I = \int_{0}^{1} \frac{ x\arctan(x) - \frac{1}{2} \ln(1+x^2) }{\sqrt{1-x^2}} dx
\]

Let’s split up:
\[
I = \int_{0}^{1} \frac{ x\arctan(x) }{\sqrt{1-x^2}} dx
-
\frac{1}{2} \int_{0}^{1} \frac{ \ln(1+x^2) }{\sqrt{1-x^2}} dx
\]


### Step 2: Reduce each integral

Let’s denote:
- \( A = \int_{0}^{1} \frac{ x \arctan(x) }{\sqrt{1-x^2}} dx \)
- \( B = \int_{0}^{1} \frac{ \ln(1+x^2) }{\sqrt{1-x^2}} dx \)

So \( I = A - \frac{1}{2} B \)

#### Compute \( A \):

Let’s use substitution \( x = \sin\theta \), \( dx = \cos\theta d\theta \), when \( x=0 \Rightarrow \theta=0 \), \( x=1\Rightarrow \theta = \frac{\pi}{2} \):

\[
A = \int_{x=0}^{x=1} \frac{x\arctan(x)}{\sqrt{1-x^2}} dx
= \int_{\theta=0}^{\frac{\pi}{2}} \frac{\sin\theta \arctan(\sin\theta)}{\cos\theta} \cdot \cos\theta d\theta
= \int_{0}^{\frac{\pi}{2}} \sin\theta \arctan(\sin\theta) d\theta
\]

#### Compute \( B \):

Again \( x = \sin\theta \), \( dx = \cos\theta d\theta \):

\[
B = \int_{x=0}^{x=1} \frac{\ln(1+x^2)}{\sqrt{1-x^2}} dx
= \int_{\theta=0}^{\frac{\pi}{2}} \frac{\ln(1+\sin^2\theta)}{\cos\theta} \cdot \cos\theta d\theta
= \int_{0}^{\frac{\pi}{2}} \ln(1+\sin^2\theta) d\theta
\]

Therefore, the original integral can be written as:
\[
I = \int_{0}^{\frac{\pi}{2}} \sin\theta\, \arctan(\sin\theta)\, d\theta - \frac{1}{2} \int_{0}^{\frac{\pi}{2}} \ln(1+\sin^2\theta) d\theta
\]

---

#### Let’s denote:

\[
I = I_1 - \frac{1}{2} I_2
\]
where
\[
I_1 = \int_{0}^{\frac{\pi}{2}} \sin\theta \arctan(\sin\theta) d\theta
\]
\[
I_2 = \int_{0}^{\frac{\pi}{2}} \ln(1+\sin^2\theta) d\theta
\]

---

### Step 3: Try to express \( I_2 \) exactly

From standard tables:

\[
\int_{0}^{\frac{\pi}{2}} \ln(1 + a^2 \sin^2 \theta)\, d\theta = \pi \ln\left(\frac{1 + \sqrt{1 + a^2}}{2}\right),\qquad a^2 \ge 0
\]

In our case, \( a^2 = 1 \). Hence,

\[
I_2 = \pi \ln\left( \frac{1 + \sqrt{2} }{2} \right)
\]

---

### Step 4: Express \( I_1 \) exactly

Let \( J(a) = \int_{0}^{\frac{\pi}{2}} \sin\theta \arctan(a \sin\theta) d\theta \)  
For \( a = 1 \), this is our \( I_1 \).  
Let’s see if this can be expressed in closed form for \( a = 1 \).

Let’s try integration by parts:
Set
- \( u = \arctan(\sin\theta), \quad dv = \sin\theta d\theta \)
- \( du = \frac{ \cos\theta }{ 1 + (\sin\theta)^2 } d\theta \)
- \( v = -\cos\theta \)

So,
\[
I_1 = u v \bigg|_{0}^{\frac{\pi}{2}} - \int_{0}^{\frac{\pi}{2}} v du
\]
\[
= \arctan(\sin\theta) (-\cos\theta)\bigg|_{0}^{\frac{\pi}{2}} + \int_{0}^{\frac{\pi}{2}} \cos\theta \cdot \frac{\cos\theta}{1 + \sin^2\theta} d\theta
\]

Let’s simplify boundary term:
- At \( \theta = 0 \): \( \arctan(0) = 0, \cos(0) = 1 \) ⇒ \( 0 \)
- At \( \theta = \frac{\pi}{2} \): \( \sin(\frac{\pi}{2}) = 1 \), \( \arctan(1) = \frac{\pi}{4} \), \( \cos(\frac{\pi}{2}) = 0 \) ⇒ \( 0 \)

So the boundary term is zero. Thus,
\[
I_1 = \int_{0}^{\frac{\pi}{2}} \frac{\cos^2\theta}{1 + \sin^2\theta} d\theta
\]

Use \( \cos^2\theta = 1 - \sin^2\theta \), so:
\[
I_1 = \int_{0}^{\frac{\pi}{2}} \frac{1-\sin^2\theta}{1+\sin^2\theta} d\theta
= \int_{0}^{\frac{\pi}{2}} \frac{1}{1+\sin^2\theta} d\theta
- \int_{0}^{\frac{\pi}{2}} \frac{\sin^2\theta}{1+\sin^2\theta} d\theta
\]
But
\[
\frac{\sin^2\theta}{1+\sin^2\theta} = 1 - \frac{1}{1+\sin^2\theta}
\]
Therefore,
\[
I_1 = \int_{0}^{\frac{\pi}{2}} \frac{1}{1+\sin^2\theta}d\theta - \left( \int_{0}^{\frac{\pi}{2}} 1 d\theta - \int_{0}^{\frac{\pi}{2}} \frac{1}{1+\sin^2\theta}d\theta \right )
\]
\[
= 2 \int_{0}^{\frac{\pi}{2}} \frac{1}{1+\sin^2\theta}d\theta - \frac{\pi}{2}
\]

Let
\[
K = \int_{0}^{\frac{\pi}{2}} \frac{1}{1+\sin^2\theta}d\theta
\]
Then
\[
I_1 = 2K - \frac{\pi}{2}
\]

Let’s compute \( K \):

#### Computation of \( K \):

Let’s try to find a closed form for

\[
K = \int_{0}^{\frac{\pi}{2}} \frac{1}{1 + \sin^2 \theta} d\theta
\]

Let’s use the Weierstrass substitution, \( t = \tan(\theta/2) \), \( \sin\theta = \frac{2t}{1 + t^2} \), \( d\theta = \frac{2dt}{1 + t^2} \).

Alternatively, let’s recall that this integral is a standard elliptic integral.  
From Gradshteyn & Ryzhik formula 3.621:

\[
\int \frac{d\theta}{1 + k^2 \sin^2\theta} = \frac{1}{\sqrt{1 + k^2}} \arctan \left( \sqrt{1 + k^2}\tan\theta \right )
\]
But that applies for \( k^2 > 0 \), duration? Let's check carefully.

Alternatively, let's try the substitution \( x = \tan\theta \), \( \theta \in [0, \frac{\pi}{2}) \) corresponds to \( x \in [0, +\infty) \), \( \sin\theta = \frac{x}{\sqrt{1 + x^2}} \), \( \cos\theta = \frac{1}{\sqrt{1 + x^2}} \), \( d\theta = \frac{dx}{1 + x^2} \).

Then:
\[
K = \int_{x=0}^{\infty} \frac{1}{1 + \left( \frac{x}{\sqrt{1 + x^2}} \right )^2 } \cdot \frac{dx}{1 + x^2}
= \int_{0}^{\infty} \frac{1}{1 + \frac{x^2}{1 + x^2}} \cdot \frac{dx}{1 + x^2 }
= \int_{0}^{\infty} \frac{1}{\frac{1 + x^2 + x^2}{1 + x^2} } \cdot \frac{dx}{1 + x^2 }
= \int_{0}^{\infty} \frac{1 + x^2}{1 + 2x^2} \cdot \frac{dx}{1 + x^2 }
\]
So:
\[
K = \int_{0}^{\infty} \frac{1}{1 + 2x^2} dx
\]
This is a simple arctangent integral:
\[
\int_{0}^{\infty} \frac{1}{1 + a^2 x^2} dx = \frac{1}{a} \arctan(a x) \Big|_{0}^{\infty} = \frac{\pi}{2a}
\]
where \( a = \sqrt{2} \).

So:
\[
K = \int_{0}^{\infty} \frac{1}{1 + 2x^2}dx = \frac{1}{\sqrt{2}} \arctan(\sqrt{2} x)\bigg|_{0}^{\infty}
\]
As \( x \rightarrow \infty \), \( \arctan(\sqrt{2} x) \to \frac{\pi}{2} \):
\[
K = \frac{1}{\sqrt{2}} \cdot \frac{\pi}{2}
\]
Thus
\[
K = \frac{\pi}{2\sqrt{2}}
\]
Therefore,
\[
I_1 = 2 \cdot \frac{\pi}{2\sqrt{2}} - \frac{\pi}{2} = \frac{\pi}{\sqrt{2}} - \frac{\pi}{2}
\]

---

### Summing up

Recall that:
\[
I = I_1 - \frac{1}{2} I_2 = \left( \frac{\pi}{\sqrt{2}} - \frac{\pi}{2} \right ) - \frac{1}{2}\pi \ln\left( \frac{1 + \sqrt{2}}{2} \right )
\]

Or:

\[
\boxed{
I = \frac{\pi}{\sqrt{2}} - \frac{\pi}{2} - \frac{\pi}{2} \ln\left( \frac{1 + \sqrt{2}}{2} \right )
}
\]

---

### Step 5: Numerical value

Let’s compute numerically (rounded to 10 decimal places):

- \( \pi \approx 3.1415926536 \)
- \( \sqrt{2} \approx 1.4142135624 \)
- \( \frac{\pi}{\sqrt{2}} \approx 3.1415926536 / 1.4142135624 \approx 2.2214414691 \)
- \( \frac{\pi}{2} \approx 1.5707963268 \)
- \( (1 + \sqrt{2})/2 = (1 + 1.4142135624)/2 = 1.2071067812 \)
- \( \ln(1.2071067812) \approx 0.1881388120 \)
- \( \frac{\pi}{2} \ln(1.2071067812) = 1.5707963268 \times 0.1881388120 \approx 0.2955448194 \)

Now compute the total:
\[
I \approx 2.2214414691 - 1.5707963268 - 0.2955448194
\]
\[
= (2.2214414691 - 1.5707963268) - 0.2955448194
\]
\[
= 0.6506451423 - 0.2955448194
\]
\[
= 0.3551003229
\]

---

## Final JSON Answer

```json
{"answer": "\\frac{\\pi}{\\sqrt{2}} - \\frac{\\pi}{2} - \\frac{\\pi}{2} \\ln \\left( \\frac{1+\\sqrt{2}}{2} \\right )", "numerical_answer": "0.3551003229"}
```