

To solve the definite integral \(\int\limits_0^2 x H_{3}\left(\sqrt{x(2-x)}\right)dx\), we follow these steps:

### Step 1: Recall the Hermite polynomial \(H_3(z)\)
The third Hermite polynomial is \(H_3(z) = 8z^3 - 12z\). Substituting \(z = \sqrt{x(2-x)}\), the integrand becomes:
\[
x H_3\left(\sqrt{x(2-x)}\right) = x \left[8\left(\sqrt{x(2-x)}\right)^3 - 12\sqrt{x(2-x)}\right] = 8x(x(2-x))^{3/2} - 12x(x(2-x))^{1/2}.
\]

### Step 2: Simplify the integral using substitution
Let \(u = x - 1\), so \(x = u + 1\) and \(dx = du\). When \(x = 0\), \(u = -1\); when \(x = 2\), \(u = 1\). The term \(x(2-x)\) simplifies to:
\[
x(2-x) = (u+1)(1 - u) = 1 - u^2.
\]
The integral splits into two parts:
\[
\int_0^2 x(x(2-x))^{3/2}dx = \int_{-1}^1 (u+1)(1 - u^2)^{3/2}du, \quad \int_0^2 x(x(2-x))^{1/2}dx = \int_{-1}^1 (u+1)(1 - u^2)^{1/2}du.
\]

### Step 3: Exploit symmetry
The integrands \((u+1)(1 - u^2)^k\) split into \(u(1 - u^2)^k + (1 - u^2)^k\). The term \(u(1 - u^2)^k\) is odd (since \(u\) is odd and \((1 - u^2)^k\) is even), so its integral over \([-1, 1]\) is zero. Thus:
\[
\int_{-1}^1 (u+1)(1 - u^2)^k du = \int_{-1}^1 (1 - u^2)^k du.
\]

### Step 4: Evaluate the remaining integrals
For \(k = 3/2\):
\[
\int_{-1}^1 (1 - u^2)^{3/2}du = 2\int_0^1 (1 - u^2)^{3/2}du.
\]
Using the substitution \(u = \sin\theta\), \(du = \cos\theta d\theta\), this becomes:
\[
2\int_0^{\pi/2} \cos^4\theta d\theta = 2 \cdot \frac{3\pi}{16} = \frac{3\pi}{8}.
\]

For \(k = 1/2\):
\[
\int_{-1}^1 (1 - u^2)^{1/2}du = 2\int_0^1 (1 - u^2)^{1/2}du.
\]
Using \(u = \sin\theta\), this becomes:
\[
2\int_0^{\pi/2} \cos^2\theta d\theta = 2 \cdot \frac{\pi}{4} = \frac{\pi}{2}.
\]

### Step 5: Combine results
The original integral is:
\[
8 \cdot \frac{3\pi}{8} - 12 \cdot \frac{\pi}{2} = 3\pi - 6\pi = -3\pi.
\]

### Numerical Approximation
The numerical value of \(-3\pi\) is approximately \(-9.4247779608\) (rounded to 10 decimal places).

{"answer": "$-3\\pi$", "numerical_answer": "-9.4247779608"}