To solve the definite integral 

\[
\int_0^{\frac{1}{2}} \left\lfloor \frac{1}{x} \right\rfloor \left\lceil \frac{1}{x} \right\rceil \ln\left(1 - \frac{1}{\left\lfloor \frac{1}{x} \right\rfloor^2}\right) \mathrm{d}x,
\]

we proceed with the following steps:

### Step 1: Understand the Integrand
The integrand involves the floor \(\left\lfloor \frac{1}{x} \right\rfloor\) and ceiling \(\left\lceil \frac{1}{x} \right\rceil\) functions, as well as a logarithmic term. 

- For \(x \in (0, \frac{1}{2}]\), \(\frac{1}{x} \in [2, \infty)\).
- The floor function \(\left\lfloor \frac{1}{x} \right\rfloor = n\) where \(n \leq \frac{1}{x} < n + 1\), which implies \(x \in \left(\frac{1}{n + 1}, \frac{1}{n}\right]\).
- The ceiling function \(\left\lceil \frac{1}{x} \right\rceil = n\) when \(x \in \left(\frac{1}{n}, \frac{1}{n - 1}\right]\), but for \(x \in \left(\frac{1}{n + 1}, \frac{1}{n}\right]\), \(\left\lceil \frac{1}{x} \right\rceil = n + 1\).

However, in the interval \(x \in \left(\frac{1}{n + 1}, \frac{1}{n}\right]\), \(\left\lfloor \frac{1}{x} \right\rfloor = n\) and \(\left\lceil \frac{1}{x} \right\rceil = n + 1\) (since \(\frac{1}{x}\) is not an integer).

### Step 2: Break the Integral into Subintervals
We partition the interval \((0, \frac{1}{2}]\) into subintervals where \(\left\lfloor \frac{1}{x} \right\rfloor\) is constant. 

For \(n \geq 2\):
- When \(x \in \left(\frac{1}{n + 1}, \frac{1}{n}\right]\), \(\left\lfloor \frac{1}{x} \right\rfloor = n\) and \(\left\lceil \frac{1}{x} \right\rceil = n + 1\).

The integral becomes:

\[
\sum_{n=2}^{\infty} \int_{\frac{1}{n + 1}}^{\frac{1}{n}} n(n + 1) \ln\left(1 - \frac{1}{n^2}\right) \mathrm{d}x.
\]

### Step 3: Simplify the Integrand
The integrand is constant over each subinterval \(\left(\frac{1}{n + 1}, \frac{1}{n}\right]\), so we can factor it out:

\[
\sum_{n=2}^{\infty} n(n + 1) \ln\left(1 - \frac{1}{n^2}\right) \left(\frac{1}{n} - \frac{1}{n + 1}\right).
\]

Simplify the difference in the integral limits:

\[
\frac{1}{n} - \frac{1}{n + 1} = \frac{1}{n(n + 1)}.
\]

Thus, the sum becomes:

\[
\sum_{n=2}^{\infty} n(n + 1) \ln\left(1 - \frac{1}{n^2}\right) \cdot \frac{1}{n(n + 1)} = \sum_{n=2}^{\infty} \ln\left(1 - \frac{1}{n^2}\right).
\]

### Step 4: Evaluate the Sum
The logarithmic term can be rewritten using the identity:

\[
\ln\left(1 - \frac{1}{n^2}\right) = \ln\left(\frac{(n - 1)(n + 1)}{n^2}\right) = \ln(n - 1) + \ln(n + 1) - 2\ln n.
\]

Now, the sum telescopes:

\[
\sum_{n=2}^{\infty} \left[\ln(n - 1) + \ln(n + 1) - 2\ln n\right].
\]

Let's write out the first few terms to observe the cancellation:

\[
\begin{align*}
&\ln(1) + \ln(3) - 2\ln(2) \\
+ &\ln(2) + \ln(4) - 2\ln(3) \\
+ &\ln(3) + \ln(5) - 2\ln(4) \\
+ &\ln(4) + \ln(6) - 2\ln(5) \\
+ &\cdots
\end{align*}
\]

Most terms cancel, leaving:

\[
\ln(1) + \ln(2) - \ln(2) - \ln(3) + \ln(3) + \ln(4) - \cdots = \ln(1) = 0.
\]

However, this is incorrect. Let's re-evaluate the telescoping behavior:

The partial sum \(S_N\) is:

\[
S_N = \sum_{n=2}^N \left[\ln(n - 1) + \ln(n + 1) - 2\ln n\right] = \ln(1) + \ln(N + 1) - \ln(2) - \ln(N).
\]

Taking the limit as \(N \to \infty\):

\[
\lim_{N \to \infty} S_N = \ln(1) - \ln(2) + \lim_{N \to \infty} \left[\ln(N + 1) - \ln(N)\right] = 0 - \ln(2) + \ln(1) = -\ln(2).
\]

Thus, the sum converges to \(-\ln(2)\).

### Step 5: Numerical Verification
The exact value is \(-\ln(2)\). Numerically:

\[
-\ln(2) \approx -0.6931471806.
\]

### Final Answer
```json
{"answer": "-\\ln(2)", "numerical_answer": "-0.6931471806"}
```