To start, note that the integrand can be rewritten as follows:
  1 + tan²x = sec²x,
so
  1/(1 + tan²x) = cos²x.

Thus, the integral becomes:
  ∫₀^(π/3) cos²x dx.

Using the power-reduction formula, cos²x can be written as:
  cos²x = (1 + cos2x)/2.

Then,
  ∫₀^(π/3) cos²x dx = (1/2)∫₀^(π/3)(1 + cos2x) dx
             = (1/2)[∫₀^(π/3) dx + ∫₀^(π/3) cos2x dx].

Computing the integrals separately:
  ∫₀^(π/3) dx = (π/3),
and
  ∫₀^(π/3) cos2x dx = (1/2)sin2x |₀^(π/3) = (1/2)[sin(2π/3) - sin0] = (1/2) sin(2π/3).

Since sin(2π/3) = √3/2, we have:
  ∫₀^(π/3) cos2x dx = (√3/4).

Thus, the overall integral becomes:
  (1/2)[(π/3) + (√3/4)] = (π/6) + (√3/8).

For the numerical approximation:
  π/6 ≈ 0.5235987756,
  √3/8 ≈ 0.2165063509,
so the sum is approximately:
  0.5235987756 + 0.2165063509 = 0.7401051265.

{"answer": "\\frac{\\pi}{6}+\\frac{\\sqrt{3}}{8}", "numerical_answer": "0.7401051265"}