
To solve the definite integral \(\int_{0}^{2} x^{-1/2}(2 - x)^{-1/2} \arcsin\left(\frac{1}{2}\sqrt{x(2 - x)}\right) \, dx\), we proceed with the following steps:


### Step 1: Substitution to Simplify the Integrand
Let \(x = 1 + \sin\theta\), so \(dx = \cos\theta \, d\theta\). When \(x = 0\), \(\theta = -\pi/2\); when \(x = 2\), \(\theta = \pi/2\). The term \(x(2 - x)\) simplifies to:
\[
x(2 - x) = (1 + \sin\theta)(1 - \sin\theta) = 1 - \sin^2\theta = \cos^2\theta.
\]
Thus, \(\sqrt{x(2 - x)} = \cos\theta\) (since \(\cos\theta \geq 0\) for \(\theta \in [-\pi/2, \pi/2]\)), and the argument of \(\arcsin\) becomes \(\frac{1}{2}\cos\theta\). The integrand simplifies as:
\[
x^{-1/2}(2 - x)^{-1/2} = \frac{1}{\sqrt{x(2 - x)}} = \frac{1}{\cos\theta}.
\]
The integral transforms to:
\[
\int_{-\pi/2}^{\pi/2} \arcsin\left(\frac{1}{2}\cos\theta\right) \, d\theta.
\]
By symmetry (the integrand is even), this becomes \(2 \int_{0}^{\pi/2} \arcsin\left(\frac{1}{2}\cos\theta\right) \, d\theta\).


### Step 2: Series Expansion of \(\arcsin\)
Using the power series for \(\arcsin(z)\) (\(|z| < 1\)):
\[
\arcsin(z) = \sum_{n=0}^{\infty} \frac{(2n)!}{4^n (n!)^2 (2n + 1)} z^{2n + 1},
\]
we substitute \(z = \frac{1}{2}\cos\theta\). The integral becomes:
\[
2 \int_{0}^{\pi/2} \sum_{n=0}^{\infty} \frac{(2n)!}{4^n (n!)^2 (2n + 1)} \left(\frac{1}{2}\cos\theta\right)^{2n + 1} d\theta.
\]
Interchanging summation and integration (justified by uniform convergence), we get:
\[
2 \sum_{n=0}^{\infty} \frac{(2n)!}{4^n (n!)^2 (2n + 1) 2^{2n + 1}} \int_{0}^{\pi/2} \cos^{2n + 1}\theta \, d\theta.
\]


### Step 3: Evaluating the Integral of \(\cos^{2n + 1}\theta\)
The integral \(\int_{0}^{\pi/2} \cos^{2n + 1}\theta \, d\theta\) is a known result from the beta function:
\[
\int_{0}^{\pi/2} \cos^{2n + 1}\theta \, d\theta = \frac{(2^n n!)^2}{(2n + 1)!}.
\]
Substituting this into the series, the terms simplify significantly, leading to:
\[
\sum_{n=0}^{\infty} \frac{1}{(2n + 1)^2 4^n}.
\]


### Step 4: Numerical Approximation
The series \(\sum_{n=0}^{\infty} \frac{1}{(2n + 1)^2 4^n}\) converges rapidly. Summing the first few terms gives:
\[
1 + \frac{1}{3^2 \cdot 4} + \frac{1}{5^2 \cdot 16} + \frac{1}{7^2 \cdot 64} + \cdots \approx 1.0306547207.
\]


### Final Answer
The exact answer is the series \(\sum_{n=0}^{\infty} \frac{1}{(2n + 1)^2 4^n}\), and the numerical approximation is approximately \(1.0306547207\).

```json
{"answer": "\\sum_{n=0}^{\\infty} \\frac{1}{(2n + 1)^2 4^n}", "numerical_answer": "1.0306547207"}
```