Let's proceed step by step.

### 1. Write the Integral

\[
I = \int_0^1 x^{-3/4}(1-x)^{-3/4}\cos\left(2\sqrt{x(1-x)}\right)dx
\]

### 2. Substitution

Let us use the substitution:
\[
x = \sin^2 \theta \implies dx = 2\sin\theta\cos\theta d\theta
\]
\[
1-x = \cos^2 \theta
\]
As \(x\) goes from 0 to 1, \(\theta\) goes from 0 to \(\pi/2\).

Plug into the integral:
\[
x^{-3/4} = (\sin^2\theta)^{-3/4} = \sin^{-3/2}\theta
\]
\[
(1-x)^{-3/4} = (\cos^2\theta)^{-3/4} = \cos^{-3/2}\theta
\]
\[
2\sqrt{x(1-x)} = 2\sqrt{\sin^2\theta \cos^2\theta} = 2\sin\theta\cos\theta = \sin 2\theta
\]
\[
dx = 2\sin\theta\cos\theta d\theta
\]

Therefore,
\[
I = \int_0^{\pi/2} \sin^{-3/2}\theta \cos^{-3/2}\theta \cos(\sin 2\theta) \cdot 2\sin\theta\cos\theta d\theta
\]

Simplify:
\[
\sin^{-3/2}\theta \cdot \sin\theta = \sin^{-1/2}\theta
\]
\[
\cos^{-3/2}\theta \cdot \cos\theta = \cos^{-1/2}\theta
\]
So:
\[
I = 2\int_0^{\pi/2} \sin^{-1/2}\theta \cos^{-1/2}\theta \cos\left(\sin 2\theta\right) d\theta
\]
But \(\sin^{-1/2}\theta \cos^{-1/2}\theta = (\sin\theta \cos\theta)^{-1/2} = \frac{1}{\sqrt{\sin\theta \cos\theta}}\)

But this is getting a bit thorny. Let's try a different approach.

Notice that:
\[
\sin\theta\cos\theta = \frac{1}{2}\sin 2\theta \implies (\sin\theta \cos\theta)^{-1/2} = 2^{1/2} (\sin 2\theta)^{-1/2}
\]
Therefore:
\[
I = 2\int_0^{\pi/2} 2^{1/2} (\sin 2\theta)^{-1/2} \cos(\sin 2\theta) d\theta
= 2^{3/2} \int_0^{\pi/2} (\sin 2\theta)^{-1/2} \cos(\sin 2\theta) d\theta
\]

Now, change variables to \(\phi = 2\theta\), so as \(\theta\) goes from 0 to \(\pi/2\), \(\phi\) goes from 0 to \(\pi\).

Also, \(d\theta = d\phi/2\).

Therefore,
\[
I = 2^{3/2}\int_{\theta=0}^{\theta=\pi/2} (\sin 2\theta)^{-1/2} \cos(\sin 2\theta)d\theta = 2^{3/2} \int_{\phi=0}^{\phi=\pi} (\sin\phi)^{-1/2} \cos(\sin\phi) \frac{d\phi}{2}
\]
\[
= 2^{1/2} \int_0^{\pi} (\sin\phi)^{-1/2} \cos(\sin\phi) d\phi
\]

So finally:
\[
I = \sqrt{2} \int_0^{\pi} \frac{\cos(\sin\phi)}{\sqrt{\sin\phi}} d\phi
\]

---

### 3. Representation in terms of Special Functions

Now, while the integral looks quite intimidating, we look for a connection to special functions.

Letâ€™s recall a certain integral representation of the Bessel function:

\[
J_{-\frac{1}{2}}(z) = \frac{1}{\pi} \int_0^{\pi} \cos(z \sin\theta) \frac{d\theta}{\sqrt{\sin\theta}}
\]
See, for instance, Gradshteyn and Ryzhik 8.431.5.

In our case, we have:

\(
\int_0^\pi \frac{\cos(a \sin\theta)}{\sqrt{\sin\theta}} d\theta = \pi J_{-1/2}(a)
\)

So for our integral, we have \(a=1\):

\[
\int_0^\pi \frac{\cos(\sin\theta)}{\sqrt{\sin\theta}} d\theta = \pi J_{-1/2}(1)
\]

Thus,

\[
I = \sqrt{2} \cdot \pi J_{-1/2}(1)
\]

---

But \(J_{-1/2}(x)\) can be written explicitly:

\[
J_{-\frac{1}{2}}(x) = \sqrt{\frac{2}{\pi x}} \cos x
\]

(see e.g. Abramowitz & Stegun, eqn 9.1.20)

So,

\[
J_{-1/2}(1) = \sqrt{\frac{2}{\pi}} \cos 1
\]

Therefore,

\[
I = \sqrt{2} \cdot \pi \cdot \sqrt{\frac{2}{\pi}} \cos 1 = \pi \sqrt{\frac{4}{\pi}} \cos 1 = 2\sqrt{\pi} \cos 1
\]

---

### 4. Numerical Value

\[
2\sqrt{\pi} \cos 1 \approx 2 \times 1.7724538509 \times 0.5403023059 \approx 1.9150896232
\]

---

### 5. Final Answer (JSON format)

```json
{"answer": "2\\sqrt{\\pi}\\cos 1", "numerical_answer": "1.9150896232"}
```