

To solve the definite integral \(\int_{0}^{2} x^{-1/2}(2 - x)^{-1/2} \cos\left(\sqrt{x(2 - x)}\right) \, dx\), we proceed as follows:

### Step 1: Simplify the integrand using substitution
First, observe that the term inside the cosine is \(\sqrt{x(2 - x)}\). Completing the square for \(x(2 - x)\), we get:
\[
x(2 - x) = 2x - x^2 = 1 - (x - 1)^2
\]
This suggests a trigonometric substitution. Let \(x - 1 = \sin\theta\), so \(x = 1 + \sin\theta\). Then:
- When \(x = 0\), \(\sin\theta = -1\) (so \(\theta = -\pi/2\)).
- When \(x = 2\), \(\sin\theta = 1\) (so \(\theta = \pi/2\)).
- \(dx = \cos\theta \, d\theta\).

Substituting \(x = 1 + \sin\theta\) into \(x(2 - x)\):
\[
x(2 - x) = (1 + \sin\theta)(1 - \sin\theta) = 1 - \sin^2\theta = \cos^2\theta
\]
Thus, \(\sqrt{x(2 - x)} = \cos\theta\) (since \(\cos\theta \geq 0\) for \(\theta \in [-\pi/2, \pi/2]\)).

### Step 2: Rewrite the integral in terms of \(\theta\)
The integrand becomes:
\[
x^{-1/2}(2 - x)^{-1/2} = \left[x(2 - x)\right]^{-1/2} = \cos^{-1}\theta
\]
The cosine term simplifies to \(\cos(\cos\theta)\). The integral then transforms to:
\[
\int_{-\pi/2}^{\pi/2} \cos^{-1}\theta \cdot \cos(\cos\theta) \cdot \cos\theta \, d\theta = \int_{-\pi/2}^{\pi/2} \cos(\cos\theta) \, d\theta
\]

### Step 3: Use symmetry and Bessel function properties
Since \(\cos(\cos\theta)\) is even (i.e., \(\cos(\cos(-\theta)) = \cos(\cos\theta)\)), we can simplify the integral:
\[
\int_{-\pi/2}^{\pi/2} \cos(\cos\theta) \, d\theta = 2 \int_{0}^{\pi/2} \cos(\cos\theta) \, d\theta
\]
Extending the interval to \([0, \pi]\) (by splitting and using symmetry), we get:
\[
2 \int_{0}^{\pi/2} \cos(\cos\theta) \, d\theta = \int_{0}^{\pi} \cos(\cos\theta) \, d\theta
\]
By the integral representation of the Bessel function \(J_0(z)\) (the Bessel function of the first kind of order 0), we know:
\[
J_0(z) = \frac{1}{\pi} \int_{0}^{\pi} \cos(z \cos\theta) \, d\theta
\]
For \(z = 1\), this becomes:
\[
\int_{0}^{\pi} \cos(\cos\theta) \, d\theta = \pi J_0(1)
\]

### Step 4: Final result
Thus, the original integral simplifies to \(\pi J_0(1)\).

### Numerical Approximation
The Bessel function \(J_0(1) \approx 0.7651976865579666\). Multiplying by \(\pi\) gives:
\[
\pi J_0(1) \approx 3.141592653589793 \times 0.7651976865579666 \approx 2.4039394433
\]

{"answer": "\(\pi J_0(1)\)", "numerical_answer": "2.4039394433"}