I'll calculate the definite integral:
$$\int_{1.0}^\infty x(x^2-1.0^2)^{2-3/2}e^{-0.5^2x^2}H_{2*2}(0.5x)dx$$

## Step 1: Simplify the expression

First, let's simplify some parts:
- $(x^2-1.0^2)^{2-3/2} = (x^2-1)^{1/2}$ since $2-3/2 = 1/2$
- $H_{2*2}(0.5x) = H_4(0.5x)$, which is the 4th Hermite polynomial

The 4th Hermite polynomial is $H_4(y) = 16y^4 - 48y^2 + 12$

So $H_4(0.5x) = 16(0.5x)^4 - 48(0.5x)^2 + 12 = 16 \cdot 0.5^4 \cdot x^4 - 48 \cdot 0.5^2 \cdot x^2 + 12$

$H_4(0.5x) = x^4 - 12x^2 + 12$

Our integral becomes:
$$\int_{1.0}^\infty x(x^2-1)^{1/2}e^{-0.25x^2}(x^4 - 12x^2 + 12)dx$$

## Step 2: Split into three integrals

Let's split this into three integrals:
$$\int_{1.0}^\infty x^5(x^2-1)^{1/2}e^{-0.25x^2}dx - 12\int_{1.0}^\infty x^3(x^2-1)^{1/2}e^{-0.25x^2}dx + 12\int_{1.0}^\infty x(x^2-1)^{1/2}e^{-0.25x^2}dx$$

## Step 3: Make a substitution

Let's use the substitution $u = x^2-1$, which gives:
- $x^2 = u+1$
- $x = \sqrt{u+1}$
- $dx = \frac{du}{2\sqrt{u+1}}$

For the first integral:
$$\int_{1.0}^\infty x^5(x^2-1)^{1/2}e^{-0.25x^2}dx = \int_{0}^\infty (u+1)^2 \cdot \sqrt{u+1} \cdot u^{1/2} \cdot e^{-0.25(u+1)} \cdot \frac{du}{2\sqrt{u+1}}$$
$$= \frac{1}{2}\int_{0}^\infty (u+1)^2 \cdot u^{1/2} \cdot e^{-0.25(u+1)}du$$
$$= \frac{1}{2}e^{-0.25}\int_{0}^\infty (u+1)^2 \cdot u^{1/2} \cdot e^{-0.25u}du$$

Similarly for the second and third integrals:

For the second integral:
$$\int_{1.0}^\infty x^3(x^2-1)^{1/2}e^{-0.25x^2}dx = \frac{1}{2}e^{-0.25}\int_{0}^\infty (u+1) \cdot u^{1/2} \cdot e^{-0.25u}du$$

For the third integral:
$$\int_{1.0}^\infty x(x^2-1)^{1/2}e^{-0.25x^2}dx = \frac{1}{2}e^{-0.25}\int_{0}^\infty u^{1/2} \cdot e^{-0.25u}du$$

## Step 4: Solve the integrals using gamma functions

For the third integral:
$$\frac{1}{2}e^{-0.25}\int_{0}^\infty u^{1/2} \cdot e^{-0.25u}du$$

This is in the form of a gamma function: $\Gamma(s) = \int_{0}^{\infty} t^{s-1}e^{-t}dt$

With the substitution $t = 0.25u$:
$$\frac{1}{2}e^{-0.25}\int_{0}^\infty u^{1/2} \cdot e^{-0.25u}du = \frac{1}{2}e^{-0.25} \cdot 4^{3/2} \cdot \Gamma(3/2)$$

Since $\Gamma(3/2) = \frac{\sqrt{\pi}}{2}$, we have:
$$\frac{1}{2}e^{-0.25} \cdot 4^{3/2} \cdot \frac{\sqrt{\pi}}{2} = \frac{1}{2}e^{-0.25} \cdot 8 \cdot \frac{\sqrt{\pi}}{2} = 2e^{-0.25} \cdot \sqrt{\pi}$$

Similarly, for the second integral:
$$\frac{1}{2}e^{-0.25}\int_{0}^\infty (u+1) \cdot u^{1/2} \cdot e^{-0.25u}du = \frac{1}{2}e^{-0.25}\left(\int_{0}^\infty u^{3/2} \cdot e^{-0.25u}du + \int_{0}^\infty u^{1/2} \cdot e^{-0.25u}du\right)$$

Using gamma functions:
$$\frac{1}{2}e^{-0.25}\left(4^{5/2} \cdot \Gamma(5/2) + 4^{3/2} \cdot \Gamma(3/2)\right)$$

Since $\Gamma(5/2) = \frac{3\sqrt{\pi}}{4}$, we have:
$$\frac{1}{2}e^{-0.25}\left(4^{5/2} \cdot \frac{3\sqrt{\pi}}{4} + 4^{3/2} \cdot \frac{\sqrt{\pi}}{2}\right) = \frac{1}{2}e^{-0.25}\left(32 \cdot \frac{3\sqrt{\pi}}{4} + 8 \cdot \frac{\sqrt{\pi}}{2}\right)$$
$$= \frac{1}{2}e^{-0.25}(24\sqrt{\pi} + 4\sqrt{\pi}) = \frac{1}{2}e^{-0.25} \cdot 28\sqrt{\pi} = 14e^{-0.25} \cdot \sqrt{\pi}$$

For the first integral:
$$\frac{1}{2}e^{-0.25}\int_{0}^\infty (u+1)^2 \cdot u^{1/2} \cdot e^{-0.25u}du = \frac{1}{2}e^{-0.25}\int_{0}^\infty (u^2 + 2u + 1) \cdot u^{1/2} \cdot e^{-0.25u}du$$
$$= \frac{1}{2}e^{-0.25}\left(\int_{0}^\infty u^{5/2} \cdot e^{-0.25u}du + 2\int_{0}^\infty u^{3/2} \cdot e^{-0.25u}du + \int_{0}^\infty u^{1/2} \cdot e^{-0.25u}du\right)$$

Using gamma functions:
$$\frac{1}{2}e^{-0.25}\left(4^{7/2} \cdot \Gamma(7/2) + 2 \cdot 4^{5/2} \cdot \Gamma(5/2) + 4^{3/2} \cdot \Gamma(3/2)\right)$$

Since $\Gamma(7/2) = \frac{15\sqrt{\pi}}{8}$:
$$\frac{1}{2}e^{-0.25}\left(4^{7/2} \cdot \frac{15\sqrt{\pi}}{8} + 2 \cdot 4^{5/2} \cdot \frac{3\sqrt{\pi}}{4} + 4^{3/2} \cdot \frac{\sqrt{\pi}}{2}\right)$$
$$= \frac{1}{2}e^{-0.25}\left(128 \cdot \frac{15\sqrt{\pi}}{8} + 2 \cdot 32 \cdot \frac{3\sqrt{\pi}}{4} + 8 \cdot \frac{\sqrt{\pi}}{2}\right)$$
$$= \frac{1}{2}e^{-0.25}(240\sqrt{\pi} + 48\sqrt{\pi} + 4\sqrt{\pi}) = \frac{1}{2}e^{-0.25} \cdot 292\sqrt{\pi} = 146e^{-0.25} \cdot \sqrt{\pi}$$

## Step 5: Combine the results

Now combining all three integrals:
$$146e^{-0.25} \cdot \sqrt{\pi} - 12 \cdot 14e^{-0.25} \cdot \sqrt{\pi} + 12 \cdot 2e^{-0.25} \cdot \sqrt{\pi}$$
$$= e^{-0.25} \cdot \sqrt{\pi}(146 - 168 + 24) = e^{-0.25} \cdot \sqrt{\pi} \cdot 2 = 2e^{-0.25} \cdot \sqrt{\pi}$$

## Step 6: Final result

The definite integral equals $2e^{-0.25} \cdot \sqrt{\pi}$

## Numerical approximation:
$2 \cdot e^{-0.25} \cdot \sqrt{\pi} = 2 \cdot 0.7788007831... \cdot 1.7724538509... = 2.7612110101...$

Rounded to 10 decimal places: 2.7612110101

{"answer": "2e^{-0.25} \\cdot \\sqrt{\\pi}", "numerical_answer": "2.7612110101"}