Let's solve the definite integral:
\[
I = \int_0^2 x\, H_3\left(\sqrt{x(2-x)}\right)dx
\]
where \( H_3(z) \) is the 3rd Hermite polynomial:
\[
H_3(z) = 8z^3 - 12z
\]
So the integral becomes:
\[
I = \int_0^2 x\, [8(\sqrt{x(2-x)})^3 - 12\sqrt{x(2-x)}] dx
\]

First, compute \((\sqrt{x(2-x)})^3 = [x(2-x)]^{3/2}\). So, the integrand is:
\[
8x[x(2-x)]^{3/2} - 12x[x(2-x)]^{1/2}
\]
Therefore,
\[
I = 8 \int_0^2 x [x(2-x)]^{3/2}dx - 12 \int_0^2 x [x(2-x)]^{1/2}dx
\]
Let’s denote:
\[
I_1 = \int_0^2 x [x(2-x)]^{3/2} dx
\]
\[
I_2 = \int_0^2 x [x(2-x)]^{1/2} dx
\]
So,
\[
I = 8 I_1 - 12 I_2
\]

---

**Step 1: Compute \(I_1 = \int_0^2 x [x(2-x)]^{3/2}dx\):**

Let’s substitute \(x = 2\sin^2 \theta\), so when \(x = 0\), \(\theta = 0\), when \(x = 2\), \(2\sin^2 \theta = 2 \implies \sin^2 \theta = 1 \implies \theta = \pi/2\).
- \(x = 2\sin^2\theta\)
- \(2-x = 2 - 2\sin^2\theta = 2\cos^2\theta\)
So,
\[
x(2-x) = 2\sin^2\theta \cdot 2\cos^2\theta = 4\sin^2\theta\cos^2\theta = 4 \sin^2\theta \cos^2\theta
\]
Therefore,
\[
[x(2-x)]^{3/2} = [4\sin^2\theta\cos^2\theta]^{3/2} = 8 \sin^3\theta \cos^3\theta
\]
Compute \(dx = 4\sin\theta\cos\theta d\theta = 2\sin 2\theta d\theta\):

\[
I_1 = \int_{\theta=0}^{\pi/2} x [x(2-x)]^{3/2} dx = \int_{0}^{\pi/2} 2\sin^2\theta \cdot 8\sin^3\theta\cos^3\theta \cdot 4\sin\theta \cos\theta d\theta
\]
Wait: But that's not getting \(dx\) right. Let's back up:

Given \(x = 2\sin^2\theta\), so
\[
dx = 4\sin\theta\cos\theta d\theta = 2\sin 2\theta d\theta
\]
So,
\[
I_1 = \int_0^2 x [x(2-x)]^{3/2} dx
= \int_{\theta=0}^{\pi/2} [2\sin^2\theta] \cdot [8\sin^3\theta\cos^3\theta] \cdot [4\sin\theta\cos\theta d\theta]
\]

Let’s expand:

- \(x = 2\sin^2\theta\)
- \([x(2-x)]^{3/2} = 8\sin^3\theta \cos^3\theta\)
- \(dx = 4\sin\theta\cos\theta d\theta\)

Therefore,
\[
I_1 = \int_0^{\pi/2} 2\sin^2\theta \cdot 8\sin^3\theta\cos^3\theta \cdot 4\sin\theta\cos\theta d\theta
\]
Multiply the constants:
\(2 \times 8 \times 4 = 64\).

The powers:
\(\sin^2\theta \sin^3\theta \sin\theta = \sin^{6}\theta\)
\(\cos^3\theta \cos\theta = \cos^{4}\theta\)

So,
\[
I_1 = 64 \int_0^{\pi/2} \sin^6\theta \cos^4\theta d\theta
\]

---

**Step 2: Compute \(I_2 = \int_0^2 x [x(2-x)]^{1/2} dx\):**

Similarly, \([x(2-x)]^{1/2} = 2\sin\theta\cos\theta\), so:

\[
I_2 = \int_0^2 x [x(2-x)]^{1/2} dx
= \int_{0}^{\pi/2} [2\sin^2\theta] \cdot [2\sin\theta\cos\theta] \cdot [4\sin\theta\cos\theta d\theta]
\]
The coefficients: \(2 \times 2 \times 4 = 16\).

The powers: \(\sin^2\theta \sin\theta \sin\theta = \sin^{4}\theta\)
\(\cos\theta \cos\theta = \cos^{2}\theta\)

So,
\[
I_2 = 16 \int_0^{\pi/2} \sin^4\theta \cos^2\theta d\theta
\]

---

**Step 3: Plug into the original integral**

Recall:
\[
I = 8I_1 - 12I_2
\]
So,
\[
I = 8 \times 64 \int_0^{\pi/2} \sin^6\theta \cos^4\theta d\theta - 12 \times 16 \int_0^{\pi/2} \sin^4\theta \cos^2\theta d\theta
\]
That is,
\[
I = 512 \int_0^{\pi/2} \sin^6\theta \cos^4\theta d\theta - 192 \int_0^{\pi/2} \sin^4\theta \cos^2\theta d\theta
\]

Let’s now compute these integrals.

---

**Step 4: Compute \(A = \int_0^{\pi/2} \sin^m\theta \cos^n\theta d\theta\)**

This is a standard Beta integral:
\[
\int_0^{\pi/2} \sin^m \theta \cos^n \theta d\theta = \frac{1}{2} \mathrm{B}\left(\frac{m+1}{2}, \frac{n+1}{2}\right)
\]

So,
\[
\int_0^{\pi/2} \sin^6\theta \cos^4\theta d\theta = \frac{1}{2} \mathrm{B}\left(\frac{7}{2}, \frac{5}{2}\right)
\]
\[
\int_0^{\pi/2} \sin^4\theta \cos^2\theta d\theta = \frac{1}{2} \mathrm{B}\left(\frac{5}{2}, \frac{3}{2}\right)
\]

Recall,
\[
\mathrm{B}(p, q) = \frac{\Gamma(p)\Gamma(q)}{\Gamma(p+q)}
\]

So,
\[
I = 512 \cdot \frac{1}{2} \mathrm{B}\left(\frac{7}{2}, \frac{5}{2}\right) - 192 \cdot \frac{1}{2} \mathrm{B}\left(\frac{5}{2}, \frac{3}{2}\right)
= 256\, \mathrm{B}\left(\frac{7}{2}, \frac{5}{2}\right) - 96\, \mathrm{B}\left(\frac{5}{2}, \frac{3}{2}\right)
\]

---

**Step 5: Write in Gamma function form**

Plug in the Beta function:

\[
I = 256\, \frac{\Gamma(7/2)\Gamma(5/2)}{\Gamma(6)} - 96\, \frac{\Gamma(5/2)\Gamma(3/2)}{\Gamma(4)}
\]

Let’s recall the basic Gamma values:

- \(\Gamma(n+1) = n! \) for integer \( n \)
- \(\Gamma(1/2) = \sqrt{\pi} \)
- \(\Gamma(3/2) = \frac{1}{2} \sqrt{\pi} \)
- \(\Gamma(5/2) = \frac{3}{4} \sqrt{\pi} \)
- \(\Gamma(7/2) = \frac{15}{8} \sqrt{\pi} \)
- \(\Gamma(4) = 3! = 6\)
- \(\Gamma(6) = 5! = 120\)

Let’s double-check those:

- \(\Gamma(x+1) = x \Gamma(x)\)
- \(\Gamma(3/2) = \frac{1}{2} \Gamma(1/2) = \frac{1}{2} \sqrt{\pi}\)
- \(\Gamma(5/2) = \frac{3}{2} \Gamma(3/2) = \frac{3}{2} \cdot \frac{1}{2} \sqrt{\pi} = \frac{3}{4} \sqrt{\pi}\)
- \(\Gamma(7/2) = \frac{5}{2}\Gamma(5/2) = \frac{5}{2} \cdot \frac{3}{4} \sqrt{\pi} = \frac{15}{8} \sqrt{\pi}\)

Correct.

Now substitute:

- \(\Gamma(7/2) = \frac{15}{8}\sqrt{\pi}\)
- \(\Gamma(5/2) = \frac{3}{4}\sqrt{\pi}\)
- \(\Gamma(3/2) = \frac{1}{2}\sqrt{\pi}\)
- \(\Gamma(6) = 120\)
- \(\Gamma(4) = 6\)

Substitute into \(I\):

First term:
\[
256 \frac{\Gamma(7/2)\Gamma(5/2)}{\Gamma(6)} = 256 \frac{\frac{15}{8}\sqrt{\pi} \cdot \frac{3}{4}\sqrt{\pi}}{120}
= 256 \frac{15 \cdot 3}{8 \cdot 4} \frac{\pi}{120}
= 256 \frac{45}{32} \frac{\pi}{120}
\]

\[
\frac{15}{8}\cdot \frac{3}{4} = \frac{45}{32},\ \ (\sqrt{\pi})^2 = \pi
\]
So numerator: \(256 \cdot 45 \cdot \pi = 11,520 \pi\)
Denominator: \(32 \cdot 120 = 3,840\)

\[
\frac{11,520 \pi}{3,840} = 3\pi
\]

Second term:

\[
96 \frac{\Gamma(5/2)\Gamma(3/2)}{\Gamma(4)} = 96 \frac{\frac{3}{4}\sqrt{\pi} \cdot \frac{1}{2}\sqrt{\pi}}{6}
= 96 \frac{3}{4} \cdot \frac{1}{2} \frac{\pi}{6}
= 96 \times \frac{3}{8} \frac{\pi}{6}
= 96 \frac{3\pi}{48}
= 96 \frac{\pi}{16}
= 6\pi
\]

Putting it all together:
\[
I = 3\pi - 6\pi = -3\pi
\]

---

**Step 6: Numerical approximation**

\[
I = -3\pi \approx -3 \cdot 3.1415926536 = -9.4247779608
\]

---

**Step 7: JSON Output**

```json
{"answer": "-3\\pi", "numerical_answer": "-9.4247779608"}
```