

To solve the definite integral \(\int_0^{2\pi}\sin(\sin(x)-x)\, dx\), we can use symmetry arguments and substitution.

### Step 1: Define the integral and use substitution
Let \( I = \int_0^{2\pi}\sin(\sin(x) - x)\, dx \). Consider the substitution \( u = 2\pi - x \). Then \( du = -dx \), and when \( x = 0 \), \( u = 2\pi \); when \( x = 2\pi \), \( u = 0 \). Rewriting the integral in terms of \( u \):

\[
I = \int_{2\pi}^0 \sin\left(\sin(2\pi - u) - (2\pi - u)\right) (-du) = \int_0^{2\pi} \sin\left(\sin(2\pi - u) - 2\pi + u\right) du
\]

### Step 2: Simplify the integrand
Using the identity \(\sin(2\pi - u) = -\sin(u)\), the argument of the sine function becomes:
\[
\sin(2\pi - u) - 2\pi + u = -\sin(u) - 2\pi + u = u - \sin(u) - 2\pi
\]

Since \(\sin(\theta - 2\pi) = \sin(\theta)\) (because sine is \(2\pi\)-periodic), we have:
\[
\sin\left(u - \sin(u) - 2\pi\right) = \sin\left(u - \sin(u)\right)
\]

Thus, the integral simplifies to:
\[
I = \int_0^{2\pi} \sin\left(u - \sin(u)\right) du
\]

### Step 3: Relate to the original integral
Notice that \(\sin(\sin(x) - x) = \sin\left(-(x - \sin(x))\right) = -\sin\left(x - \sin(x)\right)\) (since \(\sin(-\theta) = -\sin(\theta)\)). Therefore, the original integral can be rewritten as:
\[
I = \int_0^{2\pi} -\sin\left(x - \sin(x)\right) dx = -\int_0^{2\pi} \sin\left(x - \sin(x)\right) dx
\]

### Step 4: Combine results
From the substitution, we found \( I = \int_0^{2\pi} \sin\left(u - \sin(u)\right) du \), which is the same as \( \int_0^{2\pi} \sin\left(x - \sin(x)\right) dx \). Thus:
\[
I = -\int_0^{2\pi} \sin\left(x - \sin(x)\right) dx = -I
\]

This implies \( I = -I \), so \( 2I = 0 \), hence \( I = 0 \).

### Numerical Approximation
The exact value of the integral is \(0\). Rounded to 10 decimal places, the numerical approximation is \(0.0000000000\).

{"answer": "0", "numerical_answer": "0.0000000000"}