Let's compute the definite integral:
\[
I = \int_0^1 \left(e^{e^x} - e^{e^x-x}\right) dx
\]

Step 1: Split the integral:
\[
I = \int_0^1 e^{e^x} dx - \int_0^1 e^{e^x-x} dx
\]

Let’s handle each term separately.

---

### 1. Compute \(\int_0^1 e^{e^x} dx\)

Let’s use substitution:

Let \(u = e^x \implies du = e^x dx \implies dx = \frac{du}{u}\).
- When \(x = 0\), \(u = 1\)
- When \(x = 1\), \(u = e\)

So,
\[
\int_0^1 e^{e^x} dx = \int_{u=1}^{u=e} e^{u} \frac{du}{u} = \int_{1}^{e} \frac{e^{u}}{u} du
\]

---

### 2. Compute \(\int_0^1 e^{e^x-x} dx\)

Rewrite \(e^{e^x-x} = e^{e^x} e^{-x}\).

Now use the same substitution \(u = e^x\):

- \(x = 0 \implies u = 1\)
- \(x = 1 \implies u = e\)

We have: \(dx = \frac{du}{u}\), \(e^{-x} = \frac{1}{u}\)

So,
\[
\int_0^1 e^{e^x - x} dx = \int_{u=1}^{u=e} e^{u} \frac{1}{u} \frac{du}{u} = \int_1^e \frac{e^{u}}{u^2} du
\]

---

### 3. Express the answer

So,
\[
I = \int_1^e \frac{e^{u}}{u} du - \int_1^e \frac{e^{u}}{u^2} du
\]

Combine into a single integral:
\[
I = \int_1^e \left(\frac{e^{u}}{u} - \frac{e^{u}}{u^2}\right) du = \int_1^e \frac{e^{u}(u-1)}{u^2} du
\]

---

### 4. Simplify and compute the exact answer

Let’s try to get an explicit expression for this integral.

Let’s try integrating by parts or manipulating the integrand.

\[
\frac{e^{u}(u-1)}{u^2}
\]

Let’s write:
\[
\frac{u-1}{u^2} = \frac{1}{u} - \frac{1}{u^2}
\]
So:
\[
\frac{e^u(u-1)}{u^2} = \frac{e^u}{u} - \frac{e^u}{u^2}
\]

Thus, we have:
\[
I = \int_1^e \frac{e^u}{u} du - \int_1^e \frac{e^u}{u^2} du
\]

Let’s try to compute \(\int \frac{e^u}{u^2} du\).

Let’s use integration by parts:

Let:
- \(f(u) = \frac{1}{u^2}\)
- \(g(u) = e^{u}\)
then
- \(df = -\frac{2}{u^3}du\)
- \(dg = e^u du\)

Alternatively, let’s set:
Let \(v = e^u\), \(dw = \frac{1}{u^2} du\).

But perhaps it’s easier to recall that:
\[
\frac{d}{du}\left(\frac{e^u}{u}\right) = \frac{e^u}{u} - \frac{e^u}{u^2}
\]

So:
\[
\frac{e^u}{u} - \frac{e^u}{u^2} = \frac{d}{du}\left(\frac{e^u}{u}\right)
\]

Therefore, integrating:
\[
I = \int_1^e \frac{d}{du}\left(\frac{e^u}{u}\right) du = \left. \frac{e^u}{u} \right|_{u=1}^{u=e}
\]

Compute at the bounds:

- At \(u = e:\) \(\frac{e^{e}}{e} = e^{e-1}\)
- At \(u = 1:\) \(\frac{e^{1}}{1} = e\)

So,
\[
I = e^{e-1} - e
\]

---

### 5. Numerical Approximation

- \(e \approx 2.7182818285\)
- \(e^{e-1} = e^{2.7182818285 - 1} = e^{1.7182818285} \approx \exp(1.7182818285) \approx 5.5820067596\)

Subtract:
\[
I \approx 5.5820067596 - 2.7182818285 = 2.8637249311
\]

---

### Final answer in required JSON format

```json
{"answer": "e^{e-1} - e", "numerical_answer": "2.8637249311"}
```