<think>
Okay, let's see. I need to compute the definite integral from 0 to infinity of 1 over (e^x + 1) dx. Hmm, I remember that integrals involving exponentials sometimes can be simplified with substitution. Let me think.

First, the integrand is 1/(e^x + 1). Maybe I can substitute t = e^x. Let's try that. If t = e^x, then dt/dx = e^x, so dx = dt/t. When x approaches 0, t approaches 1, and as x approaches infinity, t approaches infinity. So the limits of integration from 1 to infinity. Then the integral becomes the integral from t=1 to t=∞ of 1/(t + 1) * (dt/t). Wait, that doesn't look simpler. Maybe another substitution?

Alternatively, maybe I can rewrite the integrand. Let's see, 1/(e^x + 1). If I multiply numerator and denominator by e^(-x), that gives e^(-x)/(1 + e^(-x)). So the integrand becomes e^(-x)/(1 + e^(-x)). Then maybe substitution u = 1 + e^(-x). Let's try that. Then du/dx = -e^(-x), so -du = e^(-x) dx. Then the integral becomes ∫ du/u. Let's check the limits. When x=0, u = 1 + e^0 = 2. When x approaches infinity, e^(-x) approaches 0, so u approaches 1. So the integral becomes ∫ from u=2 to u=1 of (-du)/u. Flipping the limits, that's ∫ from 1 to 2 of du/u. The integral of 1/u is ln|u|, so evaluating from 1 to 2 gives ln(2) - ln(1) = ln(2). Since ln(1) is 0. So the exact answer is ln(2). 

Wait, that seems straightforward. Let me verify. Let's do substitution again. Let u = e^(-x) + 1. Wait, no, earlier substitution was u = 1 + e^(-x). Then du = -e^(-x) dx. Wait, the integrand after substitution is e^(-x)/(1 + e^(-x)) dx. So substituting u = 1 + e^(-x), du = -e^(-x) dx. So e^(-x) dx = -du. Therefore, the integral becomes ∫ (-du)/u. The limits when x=0, u=1 + 1=2. When x→infty, u=1 + 0=1. So the integral is from u=2 to u=1 of (-du)/u, which is same as from 1 to 2 of du/u. So yes, integral is ln(2) - ln(1) = ln(2). So exact answer is ln(2). 

Alternatively, maybe another approach. Let's consider expanding 1/(e^x +1) as a series. Since e^x = sum_{n=0}^infty x^n /n! but maybe that's more complicated. Alternatively, note that 1/(e^x +1) = e^{-x}/(1 + e^{-x}) = e^{-x} * sum_{n=0}^infty (-1)^n e^{-n x} } by expanding as a geometric series, but convergence would require |e^{-x}| <1, which is true for x>0. Then integrating term by term. So integral from 0 to infinity of sum_{n=0}^\infty (-1)^n e^{-(n+1)x} dx. Then interchange sum and integral (if allowed), which would give sum_{n=0}^\infty (-1)^n ∫_0^\infty e^{-(n+1)x} dx. The integral of e^{-a x} dx from 0 to infty is 1/a. So sum_{n=0}^\infty (-1)^n / (n+1). That's sum_{k=1}^\infty (-1)^{k-1}/k, which is the alternating harmonic series, which converges to ln(2). So that also gives the same result. 

Therefore, the exact value is ln(2). Numerically, ln(2) is approximately 0.69314718056... So rounded to 10 decimal places, 0.6931471806. 

Wait, let me check the numerical value. Using calculator, ln(2) ≈ 0.6931471805599453... So rounding to 10 decimal places would be 0.6931471806. 

So the answer is ln(2) and the numerical approximation is approximately 0.6931471806.
</think>

{"answer": "\\ln(2)", "numerical_answer": "0.6931471806"}