To compute the definite integral \(\int_0^1 \frac{\ln(1+x+x^2)}{x} \, dx\), we follow these steps:

### Step 1: Simplify the Integrand
First, observe that \(1 + x + x^2\) can be factored as:
\[
1 + x + x^2 = \frac{x^3 - 1}{x - 1} \quad \text{for} \quad x \neq 1.
\]
However, this doesn't immediately simplify the integral. Instead, we consider differentiating under the integral sign or series expansion.

### Step 2: Series Expansion of the Logarithm
We use the Taylor series expansion for \(\ln(1 + x + x^2)\) around \(x = 0\):
\[
\ln(1 + x + x^2) = \sum_{n=1}^\infty \frac{(-1)^{n+1}}{n} (x + x^2)^n.
\]
Expanding \((x + x^2)^n\) and interchanging the sums (justified by uniform convergence for \(|x| < 1\)):
\[
\ln(1 + x + x^2) = \sum_{n=1}^\infty \frac{(-1)^{n+1}}{n} \sum_{k=0}^n \binom{n}{k} x^{n + k}.
\]
Thus, the integrand becomes:
\[
\frac{\ln(1 + x + x^2)}{x} = \sum_{n=1}^\infty \frac{(-1)^{n+1}}{n} \sum_{k=0}^n \binom{n}{k} x^{n + k - 1}.
\]

### Step 3: Integrate Term by Term
Integrate from 0 to 1:
\[
\int_0^1 \frac{\ln(1 + x + x^2)}{x} \, dx = \sum_{n=1}^\infty \frac{(-1)^{n+1}}{n} \sum_{k=0}^n \binom{n}{k} \int_0^1 x^{n + k - 1} \, dx.
\]
The integral evaluates to:
\[
\int_0^1 x^{n + k - 1} \, dx = \frac{1}{n + k} \quad \text{for} \quad n + k > 0.
\]
So the expression becomes:
\[
\sum_{n=1}^\infty \frac{(-1)^{n+1}}{n} \sum_{k=0}^n \binom{n}{k} \frac{1}{n + k}.
\]

### Step 4: Simplify the Double Sum
This double sum can be recognized as related to known series or integrals. Alternatively, we can use the identity:
\[
\sum_{k=0}^n \binom{n}{k} \frac{1}{n + k} = \frac{2^n}{n} \sum_{k=0}^n \frac{\binom{n}{k}}{2^k (n + k)}.
\]
However, a more straightforward approach is to consider the integral representation:
\[
\int_0^1 \frac{\ln(1 + x + x^2)}{x} \, dx = \int_0^1 \frac{\ln(1 - x^3)}{x} \, dx - \int_0^1 \frac{\ln(1 - x)}{x} \, dx.
\]
Both integrals are standard:
\[
\int_0^1 \frac{\ln(1 - x^3)}{x} \, dx = -\frac{\pi^2}{18}, \quad \int_0^1 \frac{\ln(1 - x)}{x} \, dx = -\frac{\pi^2}{6}.
\]
Thus:
\[
\int_0^1 \frac{\ln(1 + x + x^2)}{x} \, dx = -\frac{\pi^2}{18} + \frac{\pi^2}{6} = \frac{\pi^2}{9}.
\]

### Step 5: Numerical Verification
The exact value is \(\frac{\pi^2}{9}\). Numerically:
\[
\frac{\pi^2}{9} \approx 1.0966227112.
\]

### Final Answer
```json
{"answer": "\\frac{\\pi^2}{9}", "numerical_answer": "1.0966227112"}
```