Let's start by first simplifying the integral:

\[
\int_0^2 x^{(2 \cdot 1 - 1)/4}(2 - x)^{0.5/2} J_{1 - 0.5}(1 \cdot \sqrt{x}) J_{0.5}(1 \cdot \sqrt{2 - x})\, dx
\]

Plug in the parameters:

- \((2 \cdot 1 - 1)/4 = (2 - 1)/4 = 1/4\)
- \((0.5)/2 = 0.25\)
- \(J_{1 - 0.5} = J_{0.5}\)
- \(J_{0.5}\) as is.
- The arguments of the Bessel functions are \(\sqrt{x}\) and \(\sqrt{2-x}\).

So, the integral becomes:

\[
\int_0^2 x^{1/4}(2 - x)^{0.25} J_{0.5}(\sqrt{x}) J_{0.5}(\sqrt{2 - x})\, dx
\]

### 1. Analytical Evaluation

Let's use the following standard integral involving Bessel functions (see Gradshteyn & Ryzhik 6.581.3):

\[
\int_0^a x^{\mu} (a-x)^{\nu} J_{\mu}(b\sqrt{x}) J_{\nu}(c\sqrt{a-x}) dx = \frac{a^{\mu+\nu+1}(b/2)^{\mu} (c/2)^{\nu} J_{\mu+\nu+1}(\sqrt{a} \sqrt{b^2 + c^2})}{\Gamma(\mu+1)\Gamma(\nu+1)(\sqrt{a})^{\mu+\nu} \left(\sqrt{b^2 + c^2}\right)^{\mu+\nu+1}}
\]
provided \(\Re(\mu), \Re(\nu) > -1\), \(\Re(a) > 0\).

- Let \(a = 2\)
- \(\mu = 1/4\)
- \(\nu = 1/4\)
- \(b=1\), \(c=1\).

Let’s check carefully:

Plug in \(b, c\) for the Bessel function arguments:
- \(J_{\mu}(b \sqrt{x})\)
- \(J_{\nu}(c\sqrt{a-x})\)
So \(b = c = 1\).

So, the formula simplifies to:

\[
\int_0^2 x^{1/4} (2-x)^{1/4} J_{1/2}(\sqrt{x}) J_{1/2}(\sqrt{2-x}) dx = \frac{2^{1/4+1/4+1}(1/2)^{1/4}(1/2)^{1/4} J_{1/2+1/4+1/4+1}(\sqrt{2}\sqrt{1^2 + 1^2})}
{\Gamma(1/4 + 1)\Gamma(1/4 + 1) (\sqrt{2})^{1/4+1/4} (2)^{(1/4+1/4+1)}}
\]

Wait, the formula above is correct, however:
- The indices are \(\mu=\nu=1/4\), so sum in Bessel index: \(\mu+\nu+1 = 1/4+1/4+1 = 3/2\).

So plugging values:

- \(a = 2\)
- \(b = 1\), \(c = 1\)
- \(\mu = 1/4\), \(\nu = 1/4\)
- Denominator \(\Gamma(5/4)^2\)

Also, \(1^2 + 1^2 = 2\), so \(\sqrt{a}\sqrt{b^2 + c^2} = \sqrt{2} \cdot \sqrt{2} = 2\).

Evaluate numerator:
- \(a^{\mu+\nu+1} = 2^{1/4 + 1/4 + 1} = 2^{1.5} = 2\sqrt{2}\)
- \((b/2)^{\mu} = (1/2)^{1/4}\)
- \((c/2)^{\nu} = (1/2)^{1/4}\)
- \(J_{\mu+\nu+1}(2)\)

Denominator:
- \(\Gamma(1+\mu)\Gamma(1+\nu) = \Gamma(5/4)^2\)
- \((\sqrt{a})^{\mu+\nu} = (\sqrt{2})^{1/4+1/4} = (\sqrt{2})^{0.5} = 2^{0.25}\)
- \((\sqrt{b^2+c^2})^{\mu+\nu+1} = (\sqrt{2})^{1.5} = (2^{0.5})^{1.5} = 2^{0.75}\)

So compile:

Numerator:
\[
N = 2\sqrt{2} \cdot (1/2)^{1/4} \cdot (1/2)^{1/4} J_{3/2}(2) = 2\sqrt{2} \cdot (1/2)^{1/2} J_{3/2}(2)
\]
But \((1/2)^{1/2} = 1/\sqrt{2}\), so
\[
N = 2\sqrt{2} \cdot 1/\sqrt{2} J_{3/2}(2) = 2 J_{3/2}(2)
\]

Denominator:
\[
D = \Gamma(5/4)^2 \cdot 2^{0.25} \cdot 2^{0.75} = \Gamma(5/4)^2 \cdot 2^{0.25+0.75} = \Gamma(5/4)^2 \cdot 2^1 = 2 \Gamma(5/4)^2 
\]

So the exact answer is

\[
\frac{2 J_{3/2}(2)}{2 \Gamma(5/4)^2 } = \frac{J_{3/2}(2)}{\Gamma(5/4)^2}
\]

### 2. Numerical Approximation

Let’s now compute the value:

- \(J_{3/2}(2)\): Recall,
    \[
    J_{n+1/2}(x) = \sqrt{2/(\pi x)} P_n(x)
    \]
    For \(n=1\): \(J_{3/2}(x) = \sqrt{2/(\pi x)} \left(\frac{\sin x}{x} - \cos x\right)\)

So, 
\[
J_{3/2}(2) = \sqrt{\frac{2}{\pi \cdot 2}} \left( \frac{\sin 2}{2} - \cos 2 \right) = \sqrt{\frac{1}{\pi}} \left( \frac{\sin 2}{2} - \cos 2 \right)
\]

Calculate:

- \(\sin 2 \approx 0.9092974268\)
- \(\cos 2 \approx -0.4161468365\)
- \(\frac{\sin 2}{2} \approx 0.4546487134\)
- \(0.4546487134 - (-0.4161468365) = 0.4546487134 + 0.4161468365 = 0.8707955499\)
- \(\sqrt{1/\pi} \approx 0.5641895835\)

Thus,
\[
J_{3/2}(2) \approx 0.5641895835 \times 0.8707955499 \approx 0.4912931478
\]

- \(\Gamma(5/4)\):

\[
\Gamma(1.25) \approx 0.9064024771
\]
So, 
\((\Gamma(5/4))^2 \approx (0.9064024771)^2 \approx 0.8215799840\)

So the whole value is:

\[
\frac{0.4912931478}{0.8215799840} \approx 0.5979169013
\]

### 3. JSON Output

```json
{"answer": "\\frac{J_{3/2}(2)}{\\Gamma\\left(\\frac{5}{4}\\right)^2}", "numerical_answer": "0.5979169013"}
```