To solve the definite integral \(\int\limits_{0}^{2} H_{3}\left(\sqrt{x(2-x)}\right) dx\), where \(H_{3}(x)\) is the third Hermite polynomial, we follow these steps:

### Step 1: Recall the Definition of the Hermite Polynomial
The third Hermite polynomial is given by:
\[
H_{3}(x) = 8x^{3} - 12x
\]

### Step 2: Substitute the Argument
Substitute \(x\) with \(\sqrt{x(2-x)}\) in \(H_{3}(x)\):
\[
H_{3}\left(\sqrt{x(2-x)}\right) = 8\left(\sqrt{x(2-x)}\right)^{3} - 12\sqrt{x(2-x)}
\]
Simplify the expression:
\[
H_{3}\left(\sqrt{x(2-x)}\right) = 8x^{3/2}(2-x)^{3/2} - 12x^{1/2}(2-x)^{1/2}
\]

### Step 3: Split the Integral
The integral becomes:
\[
\int_{0}^{2} H_{3}\left(\sqrt{x(2-x)}\right) dx = 8 \int_{0}^{2} x^{3/2}(2-x)^{3/2} dx - 12 \int_{0}^{2} x^{1/2}(2-x)^{1/2} dx
\]

### Step 4: Use the Beta Function
The integrals can be expressed in terms of the Beta function \(B(a, b)\):
\[
\int_{0}^{2} x^{a-1}(2-x)^{b-1} dx = 2^{a+b-1} B(a, b)
\]
For the first integral (\(a = 5/2\), \(b = 5/2\)):
\[
\int_{0}^{2} x^{3/2}(2-x)^{3/2} dx = 2^{4} B\left(\frac{5}{2}, \frac{5}{2}\right)
\]
For the second integral (\(a = 3/2\), \(b = 3/2\)):
\[
\int_{0}^{2} x^{1/2}(2-x)^{1/2} dx = 2^{2} B\left(\frac{3}{2}, \frac{3}{2}\right)
\]

### Step 5: Compute the Beta Function Values
Recall that:
\[
B\left(\frac{5}{2}, \frac{5}{2}\right) = \frac{\Gamma\left(\frac{5}{2}\right)\Gamma\left(\frac{5}{2}\right)}{\Gamma(5)} = \frac{\left(\frac{3}{4}\sqrt{\pi}\right)^2}{24} = \frac{9\pi}{384} = \frac{3\pi}{128}
\]
\[
B\left(\frac{3}{2}, \frac{3}{2}\right) = \frac{\Gamma\left(\frac{3}{2}\right)\Gamma\left(\frac{3}{2}\right)}{\Gamma(3)} = \frac{\left(\frac{1}{2}\sqrt{\pi}\right)^2}{2} = \frac{\pi}{8}
\]

### Step 6: Substitute Back
Compute the integrals:
\[
8 \cdot 16 \cdot \frac{3\pi}{128} - 12 \cdot 4 \cdot \frac{\pi}{8} = 3\pi - 6\pi = -3\pi
\]

### Step 7: Numerical Approximation
The numerical value of \(-3\pi\) is approximately:
\[
-9.4247779607
\]

### Final Answer
```json
{"answer": "-3\\pi", "numerical_answer": "-9.4247779607"}
```