<think>
Okay, so I need to compute the definite integral from 1/8 to 1/4 of [ln(2x) * ln(4x) * ln(8x)] / x dx. Hmm, let's start by understanding the structure of the integrand. The integrand is a product of three logarithmic terms divided by x. The variables inside the logarithms are multiples of x: 2x, 4x, and 8x. Maybe I can simplify these logarithms first by using logarithm properties.

Let me recall that ln(ab) = ln(a) + ln(b). So, let's break down each term:

For ln(2x), that's ln(2) + ln(x). Similarly, ln(4x) is ln(4) + ln(x), and ln(8x) is ln(8) + ln(x). Let me write that out:

ln(2x) = ln(2) + ln(x) = a + t, where a = ln(2) and t = ln(x)
ln(4x) = ln(4) + ln(x) = 2a + t (since ln(4) is ln(2^2) = 2ln(2))
ln(8x) = ln(8) + ln(x) = 3a + t (since ln(8) is ln(2^3) = 3ln(2))

So substituting these into the integrand, we have:

(a + t)(2a + t)(3a + t) / x dx

But wait, the variable of integration is x, and we have t = ln(x). Let's perform a substitution to make this easier. Let me set t = ln(x). Then dt/dx = 1/x, so dt = dx/x. That means the integral becomes:

∫ [ (a + t)(2a + t)(3a + t) ] dt

But we need to adjust the limits of integration. When x = 1/8, t = ln(1/8) = -ln(8) = -3a. When x = 1/4, t = ln(1/4) = -ln(4) = -2a. Wait, let me check that:

Wait, a is ln(2), so ln(8) is ln(2^3) = 3ln(2) = 3a. Therefore, ln(1/8) = -3a, and ln(1/4) = -2a. So the limits of integration become from t = -3a to t = -2a.

So the integral simplifies to the integral from t = -3a to t = -2a of (a + t)(2a + t)(3a + t) dt. That seems more manageable. Now, let's expand the product in the integrand.

First, multiply the first two factors: (a + t)(2a + t). Let's compute that:

(a + t)(2a + t) = a*2a + a*t + t*2a + t*t = 2a² + 3a t + t²

Now, multiply this result by the third factor (3a + t):

(2a² + 3a t + t²)(3a + t) = 2a²*(3a) + 2a²*t + 3a t*(3a) + 3a t*t + t²*(3a) + t²*t

Let's compute each term:

2a²*3a = 6a³
2a²*t = 2a² t
3a t*3a = 9a² t
3a t*t = 3a t²
t²*3a = 3a t²
t²*t = t³

Combine like terms:

6a³ + (2a² t + 9a² t) + (3a t² + 3a t²) + t³
= 6a³ + 11a² t + 6a t² + t³

So the integrand becomes 6a³ + 11a² t + 6a t² + t³. Therefore, the integral is:

∫_{-3a}^{-2a} (6a³ + 11a² t + 6a t² + t³) dt

Now, let's integrate term by term.

First term: ∫6a³ dt = 6a³ t

Second term: ∫11a² t dt = 11a² * (t² / 2)

Third term: ∫6a t² dt = 6a * (t³ / 3) = 2a t³

Fourth term: ∫t³ dt = t⁴ / 4

So the antiderivative F(t) is:

6a³ t + (11a² / 2) t² + 2a t³ + (1/4) t⁴

Now, we need to evaluate this from t = -3a to t = -2a.

Compute F(-2a) - F(-3a):

First, compute F(-2a):

6a³*(-2a) + (11a² / 2)*(-2a)^2 + 2a*(-2a)^3 + (1/4)*(-2a)^4

Let's compute each term step by step.

First term: 6a³*(-2a) = -12a⁴

Second term: (11a² / 2)*(4a²) = (11a² / 2)*(4a²) = 11a² * 2a² = 22a⁴

Third term: 2a*(-8a³) = -16a⁴

Fourth term: (1/4)*(16a⁴) = 4a⁴

So adding them up:

-12a⁴ + 22a⁴ -16a⁴ +4a⁴ = (-12 + 22 -16 +4)a⁴ = (-12 -16 +22 +4)a⁴ = (-28 +26)a⁴ = (-2)a⁴

Wait, let me check that again:

First term: -12a⁴

Second term: +22a⁴

Third term: -16a⁴

Fourth term: +4a⁴

So: (-12) +22 = 10; 10 -16 = -6; -6 +4 = -2. So yes, F(-2a) = -2a⁴.

Now compute F(-3a):

6a³*(-3a) + (11a² / 2)*(-3a)^2 + 2a*(-3a)^3 + (1/4)*(-3a)^4

Compute each term:

First term: 6a³*(-3a) = -18a⁴

Second term: (11a² / 2)*(9a²) = (99a⁴)/2

Third term: 2a*(-27a³) = -54a⁴

Fourth term: (1/4)*(81a⁴) = (81/4)a⁴

Adding them up:

-18a⁴ + (99/2)a⁴ -54a⁴ + (81/4)a⁴

Convert all terms to quarters to add:

-18a⁴ = -72/4 a⁴

99/2 a⁴ = 198/4 a⁴

-54a⁴ = -216/4 a⁴

81/4 a⁴ remains as is.

So total:

(-72 + 198 -216 +81)/4 a⁴

Calculate numerator:

-72 +198 = 126; 126 -216 = -90; -90 +81 = -9

So total: (-9)/4 a⁴ = -9a⁴/4

Therefore, F(-3a) = -9a⁴/4

Thus, the integral is F(-2a) - F(-3a) = (-2a⁴) - (-9a⁴/4) = (-2 + 9/4)a⁴ = (-8/4 +9/4)a⁴ = (1/4)a⁴

So the exact value of the integral is (1/4)a⁴, where a = ln(2). Therefore, substituting back:

(1/4)(ln 2)^4

So the exact answer is (ln 2)^4 / 4.

Now, let's compute the numerical approximation. Since ln(2) is approximately 0.69314718056.

Compute (0.69314718056)^4:

First, square it: (0.69314718056)^2 ≈ 0.480453013918

Then square that result: (0.480453013918)^2 ≈ 0.480453013918 * 0.480453013918

Let me compute that:

0.48 * 0.48 = 0.2304

0.000453013918 * 0.48 ≈ 0.0002174467

0.48 * 0.000453013918 ≈ 0.0002174467

0.000453013918^2 ≈ ~0.000000205

Adding all together:

0. 0.2304 + 0.0002174467 + 0.0002174467 + 0.000000205 ≈ 0.230835098

But this is (0.480453013918)^2. So the fourth power of ln(2) is approximately 0.230835098.

Then divide by 4: 0.230835098 /4 ≈ 0.0577087745

But let me check this with a calculator for more precision.

Alternatively, use a calculator for (ln 2)^4:

ln(2) ≈ 0.6931471805599453

(ln2)^2 ≈ (0.6931471805599453)^2 ≈ 0.4804530139182014

(ln2)^4 ≈ (0.4804530139182014)^2 ≈ 0.4804530139182014 * 0.4804530139182014

Calculating this:

0.4804530139182014 * 0.4804530139182014

Let me compute this step by step:

0.4 * 0.4 = 0.16

0.4 * 0.0804530139182014 = 0.03218120556728056

0.0804530139182014 * 0.4 = 0.03218120556728056

0.0804530139182014 * 0.0804530139182014 ≈ 0.0064726500

Adding these cross terms:

0.16 + 0.03218120556728056 + 0.03218120556728056 + 0.0064726500 ≈

0.16 + 0.06436241113456112 + 0.00647265 ≈

0.16 + 0.07083506113456112 ≈ 0.23083506113456112

So (ln2)^4 ≈ 0.23083506113456112

Divide by 4: 0.23083506113456112 /4 ≈ 0.05770876528364028

Rounded to 10 decimal places: 0.0577087653

Wait, let me check with more precise calculation. Alternatively, use a calculator:

Compute ln(2) ≈ 0.6931471805599453

Compute (ln2)^4:

First, (ln2)^2: 0.6931471805599453^2 = 0.48045301391820156

Then, (0.48045301391820156)^2 = 0.2308350611345612

Divide by 4: 0.2308350611345612 /4 = 0.0577087652836403

So approximately 0.05770876528 when rounded to 10 decimal places would be 0.0577087653.

But let me check with more precise method. Let's compute 0.23083506113456112 divided by 4:

0.23083506113456112 ÷ 4:

0.23 ÷4 = 0.0575

0.00083506113456112 ÷4 = 0.00020876528364028

Adding: 0.0575 + 0.00020876528364028 = 0.05770876528364028

So yes, 0.05770876528364028, which rounds to 0.0577087653 when rounded to 10 decimal places.

Therefore, the numerical approximation is approximately 0.0577087653.

So the exact answer is (ln 2)^4 /4, which in LaTeX is \boxed{\dfrac{(\ln 2)^4}{4}} and the numerical value is approximately 0.0577087653.
</think>

{"answer": "\\dfrac{(\\ln 2)^4}{4}", "numerical_answer": 0.0577087653}