To solve the definite integral 

\[
\int_{1.0}^\infty x(x^2 - 1.0^2)^{2 - 3/2} e^{-0.5^2 x^2} H_{2*2}(0.5x) \, dx,
\]

let's break it down step by step.

### Step 1: Simplify the Integrand
First, simplify the terms in the integrand:

1. The exponent \(2 - \frac{3}{2} = \frac{1}{2}\), so \((x^2 - 1.0^2)^{\frac{1}{2}} = \sqrt{x^2 - 1}\).
2. The exponential term \(e^{-0.5^2 x^2} = e^{-0.25 x^2}\).
3. The Hermite polynomial \(H_{2*2}(0.5x) = H_4(0.5x)\). Recall that \(H_4(y) = 16y^4 - 48y^2 + 12\), so:
   \[
   H_4(0.5x) = 16(0.5x)^4 - 48(0.5x)^2 + 12 = x^4 - 12x^2 + 12.
   \]

Thus, the integrand becomes:
\[
x \sqrt{x^2 - 1} \, e^{-0.25 x^2} (x^4 - 12x^2 + 12).
\]

### Step 2: Rewrite the Integral
The integral is now:
\[
\int_{1.0}^\infty x \sqrt{x^2 - 1} \, e^{-0.25 x^2} (x^4 - 12x^2 + 12) \, dx.
\]

Let \(u = x^2 - 1\), so \(du = 2x \, dx\) and \(x \, dx = \frac{du}{2}\). When \(x = 1\), \(u = 0\), and as \(x \to \infty\), \(u \to \infty\). The integral becomes:
\[
\int_{0}^\infty \sqrt{u} \, e^{-0.25(u + 1)} \left((u + 1)^2 - 12(u + 1) + 12\right) \frac{du}{2}.
\]

Simplify the polynomial:
\[
(u + 1)^2 - 12(u + 1) + 12 = u^2 + 2u + 1 - 12u - 12 + 12 = u^2 - 10u + 1.
\]

Thus, the integral is:
\[
\frac{1}{2} \int_{0}^\infty u^{1/2} e^{-0.25u - 0.25} (u^2 - 10u + 1) \, du.
\]

Factor out \(e^{-0.25}\):
\[
\frac{e^{-0.25}}{2} \int_{0}^\infty u^{1/2} e^{-0.25u} (u^2 - 10u + 1) \, du.
\]

### Step 3: Compute the Integral
We can split the integral into three parts:
\[
\frac{e^{-0.25}}{2} \left( \int_{0}^\infty u^{5/2} e^{-0.25u} \, du - 10 \int_{0}^\infty u^{3/2} e^{-0.25u} \, du + \int_{0}^\infty u^{1/2} e^{-0.25u} \, du \right).
\]

Recall the Gamma function:
\[
\int_{0}^\infty u^{k} e^{-a u} \, du = \frac{\Gamma(k + 1)}{a^{k + 1}}.
\]

Here, \(a = 0.25\), and the exponents are \(k = \frac{5}{2}\), \(k = \frac{3}{2}\), and \(k = \frac{1}{2}\). Using \(\Gamma(n + 1) = n \Gamma(n)\) and \(\Gamma\left(\frac{1}{2}\right) = \sqrt{\pi}\), we compute:

1. For \(k = \frac{5}{2}\):
   \[
   \Gamma\left(\frac{7}{2}\right) = \frac{5}{2} \cdot \frac{3}{2} \cdot \frac{1}{2} \cdot \Gamma\left(\frac{1}{2}\right) = \frac{15}{8} \sqrt{\pi}.
   \]
   The integral is:
   \[
   \frac{\Gamma\left(\frac{7}{2}\right)}{(0.25)^{7/2}} = \frac{15 \sqrt{\pi}}{8} \cdot \frac{1}{(1/4)^{7/2}} = \frac{15 \sqrt{\pi}}{8} \cdot 4^{7/2} = \frac{15 \sqrt{\pi}}{8} \cdot 128 = 240 \sqrt{\pi}.
   \]

2. For \(k = \frac{3}{2}\):
   \[
   \Gamma\left(\frac{5}{2}\right) = \frac{3}{2} \cdot \frac{1}{2} \cdot \Gamma\left(\frac{1}{2}\right) = \frac{3}{4} \sqrt{\pi}.
   \]
   The integral is:
   \[
   \frac{\Gamma\left(\frac{5}{2}\right)}{(0.25)^{5/2}} = \frac{3 \sqrt{\pi}}{4} \cdot \frac{1}{(1/4)^{5/2}} = \frac{3 \sqrt{\pi}}{4} \cdot 32 = 24 \sqrt{\pi}.
   \]

3. For \(k = \frac{1}{2}\):
   \[
   \Gamma\left(\frac{3}{2}\right) = \frac{1}{2} \cdot \Gamma\left(\frac{1}{2}\right) = \frac{\sqrt{\pi}}{2}.
   \]
   The integral is:
   \[
   \frac{\Gamma\left(\frac{3}{2}\right)}{(0.25)^{3/2}} = \frac{\sqrt{\pi}}{2} \cdot \frac{1}{(1/4)^{3/2}} = \frac{\sqrt{\pi}}{2} \cdot 8 = 4 \sqrt{\pi}.
   \]

Now, combine the results:
\[
\frac{e^{-0.25}}{2} \left(240 \sqrt{\pi} - 10 \cdot 24 \sqrt{\pi} + 4 \sqrt{\pi}\right) = \frac{e^{-0.25}}{2} \left(240 \sqrt{\pi} - 240 \sqrt{\pi} + 4 \sqrt{\pi}\right) = \frac{e^{-0.25}}{2} \cdot 4 \sqrt{\pi} = 2 \sqrt{\pi} e^{-0.25}.
\]

### Step 4: Numerical Approximation
Compute \(2 \sqrt{\pi} e^{-0.25}\) numerically:
\[
2 \sqrt{\pi} \approx 3.5449077018, \quad e^{-0.25} \approx 0.7788007831.
\]
Multiply them:
\[
3.5449077018 \times 0.7788007831 \approx 2.760173592.
\]

### Final Answer
The exact answer is \(2 \sqrt{\pi} e^{-1/4}\), and the numerical approximation is approximately \(2.760173592\).

```json
{"answer": "2 \\sqrt{\\pi} e^{-1/4}", "numerical_answer": "2.7601735920"}
```