
To solve the definite integral \(\int_0^{\frac{1}{2}} \ln\left(\sqrt{1-x} - \sqrt{x}\right) \, dx\), we proceed as follows:


### Step 1: Simplify the integrand using trigonometric substitution
Let \(x = \sin^2\theta\), so \(dx = 2\sin\theta\cos\theta \, d\theta\). When \(x = 0\), \(\theta = 0\); when \(x = \frac{1}{2}\), \(\theta = \frac{\pi}{4}\). The integrand becomes:
\[
\sqrt{1-x} - \sqrt{x} = \cos\theta - \sin\theta = \sqrt{2}\cos\left(\theta + \frac{\pi}{4}\right),
\]
using the identity \(\cos\theta - \sin\theta = \sqrt{2}\cos\left(\theta + \frac{\pi}{4}\right)\). Thus:
\[
\ln\left(\sqrt{1-x} - \sqrt{x}\right) = \ln\left(\sqrt{2}\cos\left(\theta + \frac{\pi}{4}\right)\right) = \frac{1}{2}\ln 2 + \ln\left(\cos\left(\theta + \frac{\pi}{4}\right)\right).
\]


### Step 2: Rewrite the integral in terms of \(\theta\)
Substituting \(x = \sin^2\theta\) and \(dx = 2\sin\theta\cos\theta \, d\theta\), the integral becomes:
\[
\int_0^{\frac{\pi}{4}} \left(\frac{1}{2}\ln 2 + \ln\left(\cos\left(\theta + \frac{\pi}{4}\right)\right)\right) \cdot 2\sin\theta\cos\theta \, d\theta.
\]
This splits into two terms:
\[
\ln 2 \int_0^{\frac{\pi}{4}} \sin\theta\cos\theta \, d\theta + 2 \int_0^{\frac{\pi}{4}} \ln\left(\cos\left(\theta + \frac{\pi}{4}\right)\right) \sin\theta\cos\theta \, d\theta.
\]


### Step 3: Evaluate the first integral
The first integral is straightforward:
\[
\int_0^{\frac{\pi}{4}} \sin\theta\cos\theta \, d\theta = \frac{1}{2} \int_0^{\frac{\pi}{4}} \sin(2\theta) \, d\theta = \frac{1}{2} \left[ -\frac{\cos(2\theta)}{2} \right]_0^{\frac{\pi}{4}} = \frac{1}{4}.
\]
Thus, the first term is \(\frac{\ln 2}{4}\).


### Step 4: Evaluate the second integral
For the second integral, let \(\phi = \theta + \frac{\pi}{4}\), so \(\theta = \phi - \frac{\pi}{4}\) and \(d\theta = d\phi\). The limits change from \(\theta = 0\) to \(\phi = \frac{\pi}{4}\) and \(\theta = \frac{\pi}{4}\) to \(\phi = \frac{\pi}{2}\). The integral becomes:
\[
2 \int_{\frac{\pi}{4}}^{\frac{\pi}{2}} \ln(\cos\phi) \cdot \sin\left(\phi - \frac{\pi}{4}\right)\cos\left(\phi - \frac{\pi}{4}\right) \, d\phi.
\]
Using \(\sin\left(\phi - \frac{\pi}{4}\right)\cos\left(\phi - \frac{\pi}{4}\right) = \frac{1}{2}\sin\left(2\phi - \frac{\pi}{2}\right) = -\frac{1}{2}\cos(2\phi)\), the integral simplifies to:
\[
- \int_{\frac{\pi}{4}}^{\frac{\pi}{2}} \ln(\cos\phi) \cos(2\phi) \, d\phi.
\]


### Step 5: Integration by parts for the second integral
Let \(u = \ln(\cos\phi)\) and \(dv = \cos(2\phi) \, d\phi\). Then \(du = -\tan\phi \, d\phi\) and \(v = \frac{1}{2}\sin(2\phi)\). Integration by parts gives:
\[
\left. \frac{1}{2}\sin(2\phi)\ln(\cos\phi) \right|_{\frac{\pi}{4}}^{\frac{\pi}{2}} + \frac{1}{2} \int_{\frac{\pi}{4}}^{\frac{\pi}{2}} \sin(2\phi)\tan\phi \, d\phi.
\]
The boundary term evaluates to \(\frac{\ln 2}{4}\). The remaining integral simplifies using \(\sin(2\phi)\tan\phi = 2\sin^2\phi\), leading to:
\[
\frac{1}{2} \int_{\frac{\pi}{4}}^{\frac{\pi}{2}} 2\sin^2\phi \, d\phi = \int_{\frac{\pi}{4}}^{\frac{\pi}{2}} \sin^2\phi \, d\phi = \frac{\pi}{8} + \frac{1}{4}.
\]


### Step 6: Combine results
Combining all terms, the original integral evaluates to:
\[
\frac{\ln 2}{4} - \left( \frac{\ln 2}{4} + \frac{\pi}{8} + \frac{1}{4} \right) = -\frac{\pi + 2 + \ln 2}{4}.
\]


### Numerical Approximation
The numerical value is approximately \(-1.4586849580\).


{"answer": "-\frac{\pi + 2 + \ln 2}{4}", "numerical_answer": "-1.4586849580"}