Let's solve the definite integral:
\[
I = \int_0^{\pi/4} \frac{\tan(x) + 2\sec^2(x) + 2\tan(x)\sec^2(x)}{\tan(x) + \sec^2(x)} \; dx.
\]

**Step 1: Simplify the integrand.**

Let’s denote \( u = \tan(x) + \sec^2(x) \).

Notice that:
\[
\frac{\tan(x) + 2\sec^2(x) + 2\tan(x)\sec^2(x)}{\tan(x) + \sec^2(x)}
= \frac{[\tan(x) + \sec^2(x)] +  [\sec^2(x) + 2\tan(x)\sec^2(x)]}{\tan(x)+\sec^2(x)}
\]
But let's try combining terms in the numerator:
\[
\tan(x) + 2\sec^2(x) + 2\tan(x)\sec^2(x)
= [\tan(x) + 2\sec^2(x)] + [2\tan(x)\sec^2(x)]
\]
But maybe grouping the last two terms:
\[
\tan(x) + 2\sec^2(x) + 2\tan(x)\sec^2(x)
= \tan(x) + 2\sec^2(x) + 2\tan(x)\sec^2(x)
= \tan(x) + 2\sec^2(x)(1 + \tan(x))
\]

But \(1 + \tan(x) = \frac{\sin(x) + \cos(x)}{\cos(x)}\), but let's see another approach: maybe expand numerator in terms of denominator components.

Let's let \(A = \tan(x)\), \(B = \sec^2(x)\).
\[
\tan(x) + 2\sec^2(x) + 2\tan(x)\sec^2(x) = A + 2B + 2AB = (A + B) + (B + 2AB)
\]
So denominator is \(A + B\), so
\[
\frac{A + 2B + 2AB}{A + B} = 1 + \frac{B + 2AB}{A + B}
= 1 + \frac{B(1 + 2A)}{A + B}
\]

Let’s write \( 1 + 2A = 1 + 2\tan(x) \), \( B = \sec^2(x) \). Let's factor numerator further:
\[
I = \int_0^{\pi/4} \left[ 1 + \frac{\sec^2(x) + 2\tan(x)\sec^2(x)}{\tan(x) + \sec^2(x)} \right] dx
\]
\[
= \int_0^{\pi/4} 1 \; dx + \int_0^{\pi/4} \frac{\sec^2(x) (1 + 2\tan(x)) }{\tan(x) + \sec^2(x)} dx
\]
The first term is trivial:
\[
\int_0^{\pi/4} 1 \; dx = \frac{\pi}{4}
\]

Let’s focus on the second term:

Let’s try to write \(\tan(x) + \sec^2(x)\) in terms of \(\tan(x)\):

Recall that \(\sec^2(x) = 1+\tan^2(x)\), so:
\[
\tan(x) + \sec^2(x) = \tan(x) + 1 + \tan^2(x) = 1 + \tan(x) + \tan^2(x)
\]
So,
\[
I = \frac{\pi}{4} + \int_0^{\pi/4} \frac{(1+2\tan(x))\sec^2(x)}{1+\tan(x)+\tan^2(x)} dx
\]

Let’s use \(u = \tan(x)\), then \( du = \sec^2(x) dx \), when \( x = 0, u = 0 \), when \( x = \frac{\pi}{4}, u = 1 \):

So the integral becomes:
\[
\int_{x=0}^{x=\pi/4} \frac{(1+2\tan(x))\sec^2(x)}{1+\tan(x)+\tan^2(x)} dx = \int_{u=0}^{u=1} \frac{1+2u}{1+u+u^2} du
\]

So now our integral is:
\[
I = \frac{\pi}{4} + \int_0^{1} \frac{1+2u}{1+u+u^2} du
\]

**Step 2: Integrate \( \frac{1+2u}{1+u+u^2} \) with respect to \(u\).**

Let’s factor the denominator:
\[
1+u+u^2 = u^2 + u + 1
\]
This is not factorable over reals, so let's try to integrate:

Let’s try to write numerator as derivative of denominator plus a constant:

Let’s try:

Let’s compute the derivative of denominator:
\[
\frac{d}{du}(u^2 + u + 1) = 2u + 1
\]

Note that numerator is \(1 + 2u\), which is exactly the derivative.

Therefore:
\[
\int \frac{1+2u}{u^2 + u + 1} du = \int \frac{(u^2 + u + 1)'}{u^2 + u + 1} du = \ln|u^2 + u + 1| + C
\]

So,
\[
I = \frac{\pi}{4} + \left[ \ln(u^2 + u + 1) \right]_0^1
\]

Let’s compute the bounds:

When \(u=1\):
\[
u^2 + u + 1 = 1 + 1 + 1 = 3
\]
When \(u=0\):
\[
u^2 + u + 1 = 0 + 0 + 1 = 1
\]
Therefore,

\[
I = \frac{\pi}{4} + \left( \ln(3) - \ln(1) \right ) = \frac{\pi}{4} + \ln(3)
\]

**Step 3: Provide the numerical approximation.**

\[
I \approx \frac{\pi}{4} + \ln(3)
\]
- \( \frac{\pi}{4} \approx 0.7853981634 \)
- \( \ln(3) \approx 1.0986122887 \)
- Sum: \( 0.7853981634 + 1.0986122887 = 1.8840104521 \)

**Step 4: Output the final answer in the required JSON format**

```json
{"answer": "\\frac{\\pi}{4} + \\ln(3)", "numerical_answer": "1.8840104521"}
```