We wish to evaluate

  I = ∫₁³ [ln x/(x² + 3)] dx.

A very useful change of variable is to set

  x = √3 · t   so that dx = √3 dt.

When x = 1 we have t = 1/√3, and when x = 3 we have t = 3/√3 = √3. Also, note that

  x² + 3 = 3t² + 3 = 3(t² + 1)  and  ln x = ln(√3 t) = ln(√3) + ln t.

Thus, the integral becomes

  I = ∫ₜ₌₁/√3^(√3) [ ln(√3) + ln t ]/(3(t² + 1)) · √3 dt
    = (√3/3) · { ln(√3) ∫₁/√3^(√3) dt/(t² + 1) + ∫₁/√3^(√3) ln t/(t² + 1) dt }.

Let us call the two parts A and B:

1. A = ∫₁/√3^(√3) dt/(t² + 1).  
   This is immediate since the antiderivative of 1/(1+t²) is arctan t. Hence

  A = arctan t |ₜ₌₁/√3^(√3)
    = arctan (√3) − arctan (1/√3)
    = (π/3) − (π/6) = π/6.

2. B = ∫₁/√3^(√3) ln t/(t² + 1) dt.

Notice that if we make the substitution u = 1/t, then one finds that B changes sign (it is an odd function about the “mid‐point” on a logarithmic scale). More precisely, one can show that

  ∫₁/a^(a) ln t/(t²+1) dt = 0  for any a > 1.
In our case, a = √3, and thus B = 0.

Putting these results together we have

  I = (√3/3) [ ln(√3) · (π/6) + 0 ] 
    = (√3 π ln(√3))/(18).

Now, using ln(√3) = (1/2) ln 3, we obtain

  I = (√3 π (½ ln 3))/(18) = (π√3 ln 3)/(36).

It is sometimes preferable to write the answer in a form where the √3 is in the denominator. Multiplying numerator and denominator by √3 gives an equivalent answer:

  I = (π ln 3)/(12 √3).

Thus one acceptable exact answer is

  I = (π ln 3)/(12√3).

For a numerical check, we compute:
  π ≈ 3.1415926536,
  ln 3 ≈ 1.0986122887,
  √3 ≈ 1.7320508076.

Then
  π ln 3 ≈ 3.1415926536 × 1.0986122887 ≈ 3.451972,
and
  12√3 ≈ 12 × 1.7320508076 ≈ 20.78460969.

Thus,
  I ≈ 3.451972/20.78460969 ≈ 0.1660665600.

The final answer in the prescribed JSON format is:
{"answer": "\\frac{\\pi \\ln 3}{12\\sqrt{3}}", "numerical_answer": "0.1660665600"}