# Evaluation of $\int\limits_{0}^{4}x^{-3/4}(4-x)^{-3/4}\cosh\left(2\sqrt{x(4-x)}\right)dx$

I'll approach this integral by first analyzing its structure and making appropriate substitutions.

## Step 1: Substitution
Let's try the substitution $x = 2 - 2\cos\theta$. This gives:
- $dx = 2\sin\theta\,d\theta$
- When $x = 0$, $\cos\theta = 1$, so $\theta = 0$
- When $x = 4$, $\cos\theta = -1$, so $\theta = \pi$

Also:
- $4-x = 4 - (2 - 2\cos\theta) = 2 + 2\cos\theta$

## Step 2: Express the integrand in terms of $\theta$
Let's compute each part:

$x = 2 - 2\cos\theta$

$4-x = 2 + 2\cos\theta$

$x(4-x) = (2 - 2\cos\theta)(2 + 2\cos\theta) = 4 - 4\cos^2\theta = 4\sin^2\theta$

So $\sqrt{x(4-x)} = 2\sin\theta$

$x^{-3/4} = (2 - 2\cos\theta)^{-3/4}$

$(4-x)^{-3/4} = (2 + 2\cos\theta)^{-3/4}$

$\cosh\left(2\sqrt{x(4-x)}\right) = \cosh(4\sin\theta)$

## Step 3: Further simplification
Let's work on $x^{-3/4}(4-x)^{-3/4}$:

$x^{-3/4}(4-x)^{-3/4} = (2 - 2\cos\theta)^{-3/4}(2 + 2\cos\theta)^{-3/4}$
$= 2^{-3/4} \cdot 2^{-3/4} \cdot (1 - \cos\theta)^{-3/4} \cdot (1 + \cos\theta)^{-3/4}$
$= 2^{-3/2} \cdot (1 - \cos\theta)^{-3/4} \cdot (1 + \cos\theta)^{-3/4}$

Using the identity $(1 - \cos\theta) = 2\sin^2(\theta/2)$ and $(1 + \cos\theta) = 2\cos^2(\theta/2)$:

$x^{-3/4}(4-x)^{-3/4} = 2^{-3/2} \cdot (2\sin^2(\theta/2))^{-3/4} \cdot (2\cos^2(\theta/2))^{-3/4}$
$= 2^{-3/2} \cdot 2^{-3/4} \cdot 2^{-3/4} \cdot (\sin^2(\theta/2))^{-3/4} \cdot (\cos^2(\theta/2))^{-3/4}$
$= 2^{-3} \cdot (\sin(\theta/2))^{-3/2} \cdot (\cos(\theta/2))^{-3/2}$
$= \frac{1}{8} \cdot \frac{1}{(\sin(\theta/2))^{3/2} \cdot (\cos(\theta/2))^{3/2}}$
$= \frac{1}{8} \cdot \frac{1}{(\sin(\theta/2)\cos(\theta/2))^{3/2}}$

Using $\sin(\theta/2)\cos(\theta/2) = \frac{1}{2}\sin\theta$:

$x^{-3/4}(4-x)^{-3/4} = \frac{1}{8} \cdot \frac{1}{(\frac{1}{2}\sin\theta)^{3/2}}$
$= \frac{1}{8} \cdot \frac{2^{3/2}}{(\sin\theta)^{3/2}}$
$= \frac{1}{8} \cdot \frac{2\sqrt{2}}{(\sin\theta)^{3/2}}$
$= \frac{\sqrt{2}}{4} \cdot \frac{1}{(\sin\theta)^{3/2}}$

## Step 4: Rewrite the integral
The integral becomes:

$\int_{0}^{\pi} \frac{\sqrt{2}}{4} \cdot \frac{1}{(\sin\theta)^{3/2}} \cdot \cosh(4\sin\theta) \cdot 2\sin\theta\,d\theta$
$= \frac{\sqrt{2}}{2} \int_{0}^{\pi} \frac{\sin\theta}{(\sin\theta)^{3/2}} \cdot \cosh(4\sin\theta)\,d\theta$
$= \frac{\sqrt{2}}{2} \int_{0}^{\pi} \frac{\cosh(4\sin\theta)}{(\sin\theta)^{1/2}}\,d\theta$

## Step 5: Symmetry considerations
Due to the properties of $\sin\theta$ and $\cosh$, this integral is symmetric around $\theta = \pi/2$:

$\int_{0}^{\pi} \frac{\cosh(4\sin\theta)}{(\sin\theta)^{1/2}}\,d\theta = 2\int_{0}^{\pi/2} \frac{\cosh(4\sin\theta)}{(\sin\theta)^{1/2}}\,d\theta$

## Step 6: Use a special integral result
The integral $\int_{0}^{\pi/2} \frac{\cosh(a\sin\theta)}{(\sin\theta)^{1/2}}\,d\theta = \sqrt{\pi} \cdot I_{-1/2}(a/2)$, where $I_{-1/2}$ is the modified Bessel function of the first kind.

With $a = 4$, we get:
$\int_{0}^{\pi/2} \frac{\cosh(4\sin\theta)}{(\sin\theta)^{1/2}}\,d\theta = \sqrt{\pi} \cdot I_{-1/2}(2)$

Using the identity $I_{-1/2}(z) = \sqrt{\frac{2}{\pi z}} \cosh(z)$:
$I_{-1/2}(2) = \sqrt{\frac{2}{\pi \cdot 2}} \cosh(2) = \frac{1}{\sqrt{\pi}} \cosh(2)$

Therefore:
$\int_{0}^{\pi/2} \frac{\cosh(4\sin\theta)}{(\sin\theta)^{1/2}}\,d\theta = \sqrt{\pi} \cdot \frac{1}{\sqrt{\pi}} \cosh(2) = \cosh(2)$

## Step 7: Final calculation
Our integral is:
$\int\limits_{0}^{4}x^{-3/4}(4-x)^{-3/4}\cosh\left(2\sqrt{x(4-x)}\right)dx = \frac{\sqrt{2}}{2} \cdot 2 \cdot \cosh(2) = \sqrt{2} \cdot \cosh(2)$

Numerical approximation:
$\cosh(2) = \frac{e^2 + e^{-2}}{2} = \frac{e^2 + e^{-2}}{2} \approx 3.7621956910836$

Therefore:
$\sqrt{2} \cdot \cosh(2) \approx 1.4142135624 \cdot 3.7621956911 \approx 5.3205357280$

## Final result
$\int\limits_{0}^{4}x^{-3/4}(4-x)^{-3/4}\cosh\left(2\sqrt{x(4-x)}\right)dx = \sqrt{2} \cdot \cosh(2)$

{"answer": "\\sqrt{2} \\cdot \\cosh(2)", "numerical_answer": "5.3205357280"}