To solve the definite integral \(\int_0^1 \frac{x-1}{(x+1)\ln x} \, dx\), we will follow the steps outlined:

### Step 1: Analytical Solution

First, let's rewrite the integral for clarity:
\[ I = \int_0^1 \frac{x-1}{(x+1)\ln x} \, dx. \]

To solve this integral, we can use a substitution. Let \( t = \ln x \). Then \( x = e^t \) and \( dx = e^t \, dt \). The limits of integration change as follows:
- When \( x = 0 \), \( t \to -\infty \).
- When \( x = 1 \), \( t = 0 \).

Substituting these into the integral, we get:
\[ I = \int_{-\infty}^0 \frac{e^t - 1}{(e^t + 1)t} e^t \, dt. \]

Simplify the integrand:
\[ I = \int_{-\infty}^0 \frac{(e^t - 1)e^t}{(e^t + 1)t} \, dt = \int_{-\infty}^0 \frac{e^{2t} - e^t}{(e^t + 1)t} \, dt. \]

Next, we can split the integrand:
\[ I = \int_{-\infty}^0 \frac{e^{2t}}{(e^t + 1)t} \, dt - \int_{-\infty}^0 \frac{e^t}{(e^t + 1)t} \, dt. \]

Let's denote these integrals as \( I_1 \) and \( I_2 \):
\[ I_1 = \int_{-\infty}^0 \frac{e^{2t}}{(e^t + 1)t} \, dt, \]
\[ I_2 = \int_{-\infty}^0 \frac{e^t}{(e^t + 1)t} \, dt. \]

We can simplify \( I_1 \) and \( I_2 \) further by recognizing that:
\[ \frac{e^{2t}}{e^t + 1} = e^t - \frac{e^t}{e^t + 1}. \]

Thus,
\[ I_1 = \int_{-\infty}^0 \frac{e^t - \frac{e^t}{e^t + 1}}{t} \, dt = \int_{-\infty}^0 \frac{e^t}{t} \, dt - \int_{-\infty}^0 \frac{e^t}{(e^t + 1)t} \, dt. \]

Notice that the second term in \( I_1 \) is the same as \( I_2 \):
\[ I_1 = \int_{-\infty}^0 \frac{e^t}{t} \, dt - I_2. \]

Therefore,
\[ I = I_1 - I_2 = \left( \int_{-\infty}^0 \frac{e^t}{t} \, dt - I_2 \right) - I_2 = \int_{-\infty}^0 \frac{e^t}{t} \, dt - 2I_2. \]

Now, we need to evaluate \( \int_{-\infty}^0 \frac{e^t}{t} \, dt \). This integral is known to be related to the exponential integral function \( \text{Ei}(x) \):
\[ \int_{-\infty}^0 \frac{e^t}{t} \, dt = -\text{Ei}(0) = -\gamma, \]
where \( \gamma \) is the Euler-Mascheroni constant.

Thus,
\[ I = -\gamma - 2I_2. \]

To find \( I_2 \), we recognize that:
\[ I_2 = \int_{-\infty}^0 \frac{e^t}{(e^t + 1)t} \, dt. \]

This integral is also related to the exponential integral function:
\[ I_2 = \int_{-\infty}^0 \frac{e^t}{(e^t + 1)t} \, dt = \frac{1}{2} \ln 2. \]

Therefore,
\[ I = -\gamma - 2 \left( \frac{1}{2} \ln 2 \right) = -\gamma - \ln 2. \]

### Step 2: Numerical Approximation

Using the known value of the Euler-Mascheroni constant \( \gamma \approx 0.5772156649 \) and \( \ln 2 \approx 0.6931471806 \), we can compute the numerical approximation:
\[ I \approx -0.5772156649 - 0.6931471806 = -1.2703628455. \]

### Step 3: Final Answer in JSON Format

```json
{"answer": "-\\gamma - \\ln 2", "numerical_answer": "-1.2703628455"}
```