<think>
Okay, let's tackle this integral step by step. The integral given is ∫₀² x^(1/2)(2 - x)^(1/2) cos(1.0√(x(2 - x))) dx. Hmm, first, I need to see if there's a substitution that can simplify this expression. The integrand has x and (2 - x) under square roots, and the argument of the cosine is also involving the product x(2 - x). Maybe a substitution that simplifies the square roots would help here.

Let me consider substituting t = x(2 - x). Let's compute dt/dx. The derivative of t with respect to x is 2 - 2x. Wait, but that might complicate things because the integrand also has sqrt(x) and sqrt(2 - x). Alternatively, maybe a trigonometric substitution? Since the product x(2 - x) resembles a quadratic expression that can be rewritten in terms of a square. Let's see: x(2 - x) = 2x - x² = -(x² - 2x) = -(x² - 2x +1 -1) = -(x -1)^2 +1. So, x(2 - x) = 1 - (x -1)^2. That looks like a form suitable for a sine or cosine substitution. Let me try substituting u = x -1. Then, the expression becomes 1 - u². So, if u = sinθ, then 1 - u² = cos²θ. Let's try that.

But wait, if u = x -1, then x = u +1, and when x goes from 0 to 2, u goes from -1 to 1. Then, the integral becomes ∫_{-1}^{1} sqrt(u +1) sqrt(1 - u) cos(1.0 * sqrt(1 - u²)) du. Hmm, sqrt(u +1) * sqrt(1 - u) is sqrt((1 + u)(1 - u)) = sqrt(1 - u²). So, the integrand simplifies to sqrt(1 - u²) cos(1.0 * sqrt(1 - u²)) du. That's better. So the integral becomes ∫_{-1}^{1} sqrt(1 - u²) cos(1.0 * sqrt(1 - u²)) du.

But since the integrand is even (because sqrt(1 - u²) is even and cos(sqrt(1 - u²)) is also even), we can write this as 2 * ∫₀}^{1} sqrt(1 - u²) cos(1.0 * sqrt(1 - u²)) du. Now, let's make another substitution. Let’s set t = sqrt(1 - u²). Then, t² = 1 - u², so 2t dt = -2u du → u du = -t dt. Wait, but we need to express the integral in terms of t. Let's see:

If t = sqrt(1 - u²), then when u = 0, t = 1, and when u =1, t =0. The integral becomes 2 * ∫_{t=1}^{t=0} t cos(1.0 t) * ( -u du ). Wait, but we need to express du in terms of dt. From t = sqrt(1 - u²), dt/du = (-u)/sqrt(1 - u²) = -u/t. Therefore, du = -t/u dt. But in the integral, we have sqrt(1 - u²) du = t du. Substituting du = -t/u dt, so t du = -t*(t/u) dt = -t²/u dt. But u = sqrt(1 - t²) since u = sqrt(1 - t²) when t = sqrt(1 - u²). Wait, maybe this substitution is getting too complicated. Let me try a different approach.

Alternatively, let's let t = sqrt(1 - u²). Then, t = sqrt(1 - u²) → t² = 1 - u² → u = sqrt(1 - t²). Wait, but when u is in [0,1], t is in [0,1] as well. Wait, no: if u goes from 0 to1, then t = sqrt(1 - u²) goes from 1 to 0. So, maybe substitution variable t = sqrt(1 - u²), then dt/du = (-u)/sqrt(1 - u²) = -u/t. So, du = -t/u dt. Let's substitute into the integral:

The integral is 2 * ∫_{u=0}^{1 sqrt(1 - u²) cos(1.0 sqrt(1 - u²)) du. Let t = sqrt(1 - u²), so when u=0, t=1; u=1, t=0. Then, the integral becomes 2 * ∫_{t=1}^{t=0} t cos(1.0 t) * (-t/u) dt. But u = sqrt(1 - t²), so substituting back, we have:

2 * ∫₁⁰ t cos(t) * (-t / sqrt(1 - t²)) dt. The negative sign flips the limits:

2 * ∫₀¹ t cos(t) * (t / sqrt(1 - t²)) dt = 2 * ∫₀¹ (t² / sqrt(1 - t²)) cos(t) dt.

Hmm, this seems more complicated. Maybe this substitution isn't helpful. Let's think again.

Wait, the original substitution u = x -1 transformed the integral into 2 * ∫₀¹ sqrt(1 - u²) cos(sqrt(1 - u²)) du. Let me consider another substitution here. Let’s set θ = sqrt(1 - u²). Then, θ = sqrt(1 - u²) → θ² = 1 - u² → u² = 1 - θ² → 2θ dθ = -2u du → u du = -θ dθ. But in the integral, we have sqrt(1 - u²) du = θ du. So, substituting θ = sqrt(1 - u²), then du = -θ dθ / u. But u = sqrt(1 - θ²). So, substituting back, the integral becomes:

2 * ∫_{θ=1}^{θ=0} θ * cos(θ) * (-θ / sqrt(1 - θ²)) dθ. Again, flipping the limits:

2 * ∫₀¹ (θ² / sqrt(1 - θ²)) cos(θ) dθ. Hmm, same as before. Not helpful. Maybe another approach.

Alternatively, perhaps integrating by parts. Let's consider the integral ∫ sqrt(1 - u²) cos(sqrt(1 - u²)) du. Let’s set v = sqrt(1 - u²), then dv/du = (-u)/sqrt(1 - u²). Let’s set dw = cos(v) du. Then, w = ∫ cos(v) du. But v is a function of u, so this might not be straightforward. Alternatively, let’s set t = v = sqrt(1 - u²). Then, dt/du = -u / sqrt(1 - u²) = -u / t. So, du = -t/u dt. But u = sqrt(1 - t²). So, du = -t / sqrt(1 - t²) dt. Then, the integral becomes ∫ t cos(t) * (-t / sqrt(1 - t²)) dt. Which is the same as before. So, perhaps this is not helpful.

Wait, maybe another substitution. Let’s consider the original integral again: ∫₀² sqrt(x) sqrt(2 - x) cos(sqrt(x(2 - x))) dx. Let’s try substituting t = sqrt(x(2 - x)). Then, t² = x(2 - x) = 2x - x². Let’s compute dt/dx: dt/dx = (2 - 2x)/(2 sqrt(x(2 - x))) = (1 - x)/t. Hmm, but then we need to express the integrand in terms of t. The integrand is sqrt(x) sqrt(2 - x) cos(t) dx. But sqrt(x) sqrt(2 - x) = sqrt(x(2 - x)) = t. So, the integrand becomes t cos(t) dx. But we need to express dx in terms of dt. From t² = 2x - x², differentiating both sides: 2t dt = (2 - 2x) dx → dx = t dt / (1 - x). But x is related to t via t² = 2x - x². Let’s solve for x in terms of t. Rearranging t² = -x² + 2x → x² - 2x + t² =0. Using quadratic formula: x = [2 ± sqrt(4 -4t²)]/2 = 1 ± sqrt(1 - t²). But since x is between 0 and 2, both roots are possible. However, when x is in [0,1], the positive root is 1 + sqrt(1 - t²), but sqrt(1 - t²) is real only if t² ≤1. Wait, t = sqrt(x(2 -x)), which for x in [0,2], t ranges from 0 to 1 (since maximum of x(2 -x) is at x=1, which is 1*1=1). So t is in [0,1]. Therefore, x = 1 ± sqrt(1 - t²). But when x is in [0,2], for each t, there are two x values. However, since we're integrating from 0 to 2, perhaps we need to split the integral into two parts? Wait, but maybe this substitution complicates things because x is not a single-valued function of t. Maybe this substitution isn't the way to go.

Alternatively, let's consider a substitution that can turn the integral into a standard form. The integrand has sqrt(x(2 -x)) which is similar to the equation of a circle. Let me try substituting x = 1 + sinθ. Then, 2 - x = 1 - sinθ. Then, x(2 -x) = (1 + sinθ)(1 - sinθ) = 1 - sin²θ = cos²θ. So sqrt(x(2 -x)) = cosθ. Then, the argument of the cosine becomes 1.0 * cosθ. Also, dx = cosθ dθ. Let's check the limits. When x=0: 0 =1 + sinθ → sinθ = -1 → θ = -π/2. When x=2: 2 =1 + sinθ → sinθ=1 → θ=π/2. So the integral becomes ∫_{-π/2}^{π/2} sqrt(1 + sinθ) sqrt(1 - sinθ) cos(1.0 cosθ) * cosθ dθ. Simplify sqrt(1 + sinθ)sqrt(1 - sinθ) = sqrt(1 - sin²θ) = cosθ. So the integrand becomes cosθ * cos(cosθ) * cosθ dθ = cos²θ cos(cosθ) dθ. Therefore, the integral is ∫_{-π/2}^{π/2} cos²θ cos(cosθ) dθ. Since the integrand is even (cos²θ is even, cos(cosθ) is even), this becomes 2 * ∫₀^{π/2} cos²θ cos(cosθ) dθ.

Hmm, this seems more manageable, but integrating cos²θ cos(cosθ) dθ is still non-trivial. Let's see if we can express cos²θ in terms of a double angle identity. cos²θ = (1 + cos2θ)/2. So the integral becomes 2 * ∫₀^{π/2} (1 + cos2θ)/2 * cos(cosθ) dθ = ∫₀^{π/2} (1 + cos2θ) cos(cosθ) dθ. So, split into two integrals: ∫₀^{π/2} cos(cosθ) dθ + ∫₀^{π/2} cos2θ cos(cosθ) dθ.

Let’s consider the first integral: I₁ = ∫₀^{π/2} cos(cosθ) dθ. The second integral: I₂ = ∫₀^{π/2} cos2θ cos(cosθ) dθ. These integrals don't seem to have elementary antiderivatives. Maybe we can express them in terms of Bessel functions? Because integrals involving cos(a cosθ) often relate to Bessel functions. Let me recall that the Bessel function of the first kind J_n(z) is given by:

J_n(z) = (1/π) ∫₀^π cos(nθ - z sinθ) dθ.

But our integrals involve cos(cosθ) and cos2θ cos(cosθ). Let me see if there's a relation. Alternatively, expand cos(cosθ) in a Fourier series or a Taylor series.

Alternatively, expand cos(cosθ) as a Taylor series: cos(cosθ) = Σ_{k=0}^∞ (-1)^k (cosθ)^{2k}/(2k)!.

Then, integrating term by term. Let's try that.

First, expand cos(cosθ):

cos(cosθ) = Σ_{k=0}^∞ [ (-1)^k / (2k)! ) ] (cosθ)^{2k}

Then, I₁ = ∫₀^{π/2} Σ_{k=0}^∞ [ (-1)^k / (2k)! ) ] (cosθ)^{2k} dθ = Σ_{k=0}^∞ [ (-1)^k / (2k)! ) ] ∫₀^{π/2} (cosθ)^{2k} dθ.

Similarly, the integral of (cosθ)^{2k} from 0 to π/2 is known as the beta function or using the formula:

∫₀^{π/2} cos^{2k}θ dθ = (π/2) ( (2k)! ) / (4^k (k!)^2 )

This is the Wallis integral. So, substituting back:

I₁ = Σ_{k=0}^∞ [ (-1)^k / (2k)! ) ] * (π/2) * ( (2k)! ) / (4^k (k!)^2 ) ) = (π/2) Σ_{k=0}^∞ [ (-1)^k / (4^k (k!)^2 ) ]

This series is known. Let's recognize that Σ_{k=0}^∞ [ (-1)^k / (k!^2 ) ] (x/4)^k is the series expansion of the Bessel function of the first kind J_0(√x). Wait, more precisely, J_0(z) = Σ_{k=0}^∞ [ (-1)^k / (k!^2 ) ] (z/2)^{2k}. So, if we set z = 2, then J_0(2) = Σ_{k=0}^∞ [ (-1)^k / (k!^2 ) ] (2/2)^{2k} = Σ_{k=0}^∞ [ (-1)^k / (k!^2 ) ] 1^k = Σ_{k=0}^∞ [ (-1)^k / (k!^2 ) ].

But our series is Σ_{k=0}^∞ [ (-1)^k / (4^k (k!)^2 ) ] = Σ_{k=0}^∞ [ (-1)^k / (k!^2 ) ] (1/4)^k. Comparing to J_0(z), which is Σ_{k=0}^∞ [ (-1)^k / (k!^2 ) ] (z/2)^{2k} = Σ_{k=0}^∞ [ (-1)^k / (k!^2 ) ] (z²/4)^k. So, if we set z²/4 = 1/4 → z²=1 → z=1. Therefore, Σ_{k=0}^∞ [ (-1)^k / (4^k (k!)^2 ) ] = J_0(1). Therefore, I₁ = (π/2) J_0(1).

Similarly, let's compute I₂ = ∫₀^{π/2} cos2θ cos(cosθ) dθ. Again, expand cos(cosθ) as a series:

I₂ = ∫₀^{π/2} cos2θ Σ_{k=0}^∞ [ (-1)^k / (2k)! ) ] (cosθ)^{2k} dθ = Σ_{k=0}^∞ [ (-1)^k / (2k)! ) ] ∫₀^{π/2} cos2θ (cosθ)^{2k} dθ.

We need to evaluate ∫₀^{π/2} cos2θ (cosθ)^{2k} dθ. Let's use substitution or look for a known integral. Let’s consider writing cos2θ in terms of cosines. Alternatively, use integration by parts. Let’s set u = cos2θ, dv = (cosθ)^{2k} dθ. But this might not be helpful. Alternatively, use the identity cos2θ = 2cos²θ -1. Then,

∫ cos2θ (cosθ)^{2k} dθ = ∫ (2cos²θ -1)(cosθ)^{2k} dθ = 2 ∫ (cosθ)^{2k +2} dθ - ∫ (cosθ)^{2k} dθ.

Therefore, the integral becomes 2 * I(k+1) - I(k), where I(n) = ∫₀^{π/2} (cosθ)^{2n} dθ = (π/2) ( (2n)! ) / (4^n (n!)^2 )

Therefore, substituting back:

∫₀^{π/2} cos2θ (cosθ)^{2k} dθ = 2*(π/2)*( (2(k+1))! ) / (4^{k+1} ( (k+1)! )^2 ) ) - (π/2)*( (2k)! ) / (4^k (k!)^2 )

Simplify:

= π/2 [ 2*( (2k + 2)! ) / (4^{k+1} ( (k+1)! )^2 ) ) - ( (2k)! ) / (4^k (k!)^2 ) ]

= π/2 [ ( (2k + 2)! ) / (4^{k} ( (k+1)! )^2 * 2 ) ) - ( (2k)! ) / (4^k (k!)^2 ) ]

Wait, let's compute each term:

First term: 2 * I(k+1) = 2 * (π/2) * ( (2(k+1))! ) / (4^{k+1} ( (k+1)! )^2 ) ) = π * (2(k+1))! / (4^{k+1} ( (k+1)! )^2 )

Second term: -I(k) = - (π/2) * (2k)! / (4^k (k!)^2 )

So, the integral is π * (2k + 2)! / (4^{k+1} ( (k+1)! )^2 ) - (π/2) * (2k)! / (4^k (k!)^2 )

Let’s factor out π / (4^{k} (k!)^2 ):

= π / (4^{k} (k!)^2 ) [ ( (2k + 2)! ) / (4 * ( (k+1)! )^2 ) ) - (1/2) (2k)! ) ]

Note that (2k + 2)! = (2k + 2)(2k +1)(2k)! )

And (k+1)! )^2 = (k+1)^2 (k! )^2 )

So, substituting:

= π / (4^{k} (k! )^2 ) [ ( (2k + 2)(2k +1)(2k)! ) / (4 * (k+1)^2 (k! )^2 ) ) - (1/2)(2k)! / (k! )^2 ) ]

Simplify the first term inside the brackets:

= [ (2k + 2)(2k +1) / (4 (k+1)^2 ) ) * (2k)! / (k! )^2 ) ] - (1/2)(2k)! / (k! )^2 )

Factor out (2k)! / (k! )^2 ):

= (2k)! / (k! )^2 ) [ (2k +2)(2k +1)/(4 (k+1)^2 ) - 1/2 ]

Simplify the expression inside the brackets:

First term: (2k +2)(2k +1) = 2(k +1)(2k +1)

Denominator: 4(k+1)^2

So, first fraction: [2(k+1)(2k +1)] / [4(k+1)^2] = (2k +1)/(2(k+1))

So, the expression becomes:

(2k +1)/(2(k+1)) - 1/2 = [ (2k +1) - (k +1) ] / (2(k+1)) ) = (k) / (2(k+1))

Therefore, the entire expression becomes:

= (2k)! / (k! )^2 ) * (k) / (2(k+1)) )

= (2k)! * k ) / ( 2(k+1) (k! )^2 )

But (2k)! / (k! )^2 ) = C(2k, k), the binomial coefficient. So,

= C(2k, k) * k / (2(k+1))

Therefore, the integral ∫₀^{π/2} cos2θ (cosθ)^{2k} dθ = π / (4^{k} (k! )^2 ) * C(2k, k) * k / (2(k+1)) )

But C(2k, k) = (2k)! / (k! )^2, so substituting back:

= π / (4^{k} (k! )^2 ) * ( (2k)! / (k! )^2 ) * k / (2(k+1)) )

= π (2k)! k / (4^{k} (k! )^4 * 2(k+1)) )

This seems very complicated. Maybe there's a simpler way to express this. Alternatively, perhaps this approach is not the best. Let's consider another way.

Alternatively, recall that the integral I₂ can be expressed in terms of derivatives of Bessel functions. Let me recall that integrals involving cos(nθ) cos(a cosθ) can be related to Bessel functions. For example, the integral ∫₀^π cos(nθ) cos(a cosθ) dθ is related to Bessel functions. Specifically, there's an identity:

∫₀^π cos(nθ) cos(a cosθ) dθ = π (-1)^n J_n(a)

But I need to verify this. Wait, let me check standard integrals. The standard integral is:

∫₀^π cos(nθ - z sinθ) dθ = π J_n(z)

But this is different from our case. Alternatively, expanding cos(a cosθ) in terms of Bessel functions. There's an expansion known as the Jacobi-Anger expansion, but that usually involves exponentials. Alternatively, using the identity:

cos(a cosθ) = J_0(a) + 2 Σ_{k=1}^∞ (-1)^k J_{2k}(a) cos(2kθ)

This is a Fourier series expansion. Therefore, substituting this into I₂:

I₂ = ∫₀^{π/2} cos2θ [ J_0(1) + 2 Σ_{k=1}^∞ (-1)^k J_{2k}(1) cos(2kθ) ] dθ

= J_0(1) ∫₀^{π/2} cos2θ dθ + 2 Σ_{k=1}^∞ (-1)^k J_{2k}(1) ∫₀^{π/2} cos2θ cos(2kθ) dθ

Compute the first integral: ∫₀^{π/2} cos2θ dθ = [ sin2θ / 2 ] from 0 to π/2 = (sinπ - sin0)/2 = 0.

The second integral: ∫₀^{π/2} cos2θ cos(2kθ) dθ. Using orthogonality of cosines, this is zero unless 2k = 2, i.e., k=1. For k=1, the integral becomes ∫₀^{π/2} cos²2θ dθ = π/4. For other k, it's zero. Wait, let's compute it properly.

Using the identity cosA cosB = [cos(A+B) + cos(A-B)]/2.

So, cos2θ cos(2kθ) = [cos(2θ + 2kθ) + cos(2θ - 2kθ)]/2 = [cos(2(k+1)θ) + cos(2(k-1)θ)]/2.

Integrate from 0 to π/2:

= 1/2 [ ∫₀^{π/2} cos(2(k+1)θ) dθ + ∫₀^{π/2} cos(2(k-1)θ) dθ ]

For the first integral: ∫ cos(2(k+1)θ) dθ from 0 to π/2:

= [ sin(2(k+1)θ)/(2(k+1)) ] from 0 to π/2 = [ sin((k+1)π) - sin0 ]/(2(k+1)) = 0, since sin(nπ) =0 for integer n.

Similarly, the second integral: ∫ cos(2(k-1)θ) dθ from 0 to π/2:

= [ sin(2(k-1)θ)/(2(k-1)) ] from 0 to π/2 = [ sin((k-1)π) - sin0 ]/(2(k-1)) = 0, unless k=1.

If k=1, the second integral becomes ∫₀^{π/2} cos(0θ) dθ = ∫₀^{π/2} 1 dθ = π/2.

Therefore, for k=1:

∫₀^{π/2} cos2θ cos(2*1θ) dθ = 1/2 [ 0 + π/2 ] = π/4.

For k≠1, the integral is zero.

Therefore, I₂ = 0 + 2 Σ_{k=1}^∞ (-1)^k J_{2k}(1) * (π/4) δ_{k,1} } = 2 * (-1)^1 J_2}(1) * π/4 = -2 * J_2(1) * π/4 = -π/2 J_2(1).

Therefore, combining I₁ and I₂:

The original integral is I = I₁ + I₂ = (π/2) J_0(1) - (π/2) J_2(1) = (π/2)( J_0(1) - J_2(1) ).

But there's a recurrence relation for Bessel functions: J_{n-1}(x) + J_{n+1}(x) = (2n/x) J_n(x). For x=1 and n=1: J_0(1) + J_2(1) = 2*1/1 J_1(1) → J_0(1) + J_2(1) = 2 J_1(1). Therefore, J_0(1) - J_2(1) = 2 J_1(1) - 2 J_2(1) ? Wait, no. Let's solve for J_0(1) - J_2(1):

From J_0(1) + J_2(1) = 2 J_1(1), we have J_0(1) - J_2(1) = 2 J_1(1) - 2 J_2(1). Hmm, not helpful. Wait, perhaps another recurrence relation. Alternatively, using the identity J_{n-1}(x) - J_{n+1}(x) = 2 J_n'(x). For n=1: J_0(x) - J_2(x) = 2 J_1'(x). But J_1'(x) = (J_0(x) - J_2(x))/2. However, integrating this might not help. Alternatively, for x=1, J_0(1) - J_2(1) = 2 J_1'(1). But I'm not sure if this helps in simplifying the expression.

Alternatively, we can leave the answer in terms of Bessel functions. Therefore, the original integral is equal to (π/2)( J_0(1) - J_2(1) ).

But let's verify this. Let me check with numerical integration. Suppose we compute the original integral numerically and compare with (π/2)( J_0(1) - J_2(1) ).

First, compute J_0(1), J_2(1). The values of Bessel functions at 1 are known:

J_0(1) ≈ 0.7651976865

J_1(1) ≈ 0.4400505857

J_2(1) ≈ 0.1149034849

Therefore, J_0(1) - J_2(1) ≈ 0.7651976865 - 0.1149034849 ≈ 0.6502942016

Multiply by π/2 ≈ 1.5707963268 * 0.6502942016 ≈ 1.021657382

But let's compute the original integral numerically. The integral is ∫₀² sqrt(x) sqrt(2 -x) cos(sqrt(x(2 -x))) dx.

Let’s approximate this using numerical methods. Let's use substitution x = 1 + u, then the integral becomes ∫_{-1}^{1} sqrt(1 + u) sqrt(1 - u) cos(sqrt(1 - u²)) du. Which is 2 ∫₀¹ sqrt(1 - u²) cos(sqrt(1 - u²)) du. Let’s approximate this integral numerically. Let's use a numerical integration method like Simpson's rule with a sufficient number of intervals.

Alternatively, use a calculator or software. But since I need to approximate this manually, let's take a few sample points. However, this might not be accurate. Alternatively, recall that we transformed the integral into (π/2)( J_0(1) - J_2(1) ). Using the values:

π/2 ≈ 1.5707963268

J_0(1) ≈ 0.7651976865

J_2(1) ≈ 0.1149034849

So, 0.7651976865 - 0.1149034849 = 0.6502942016

Multiply by π/2: 0.6502942016 * 1.5707963268 ≈ 1.021657382

So, the exact answer is (π/2)( J₀(1) - J₂(1) ), and the numerical approximation is approximately 1.021657382. Let's check with a numerical integration.

Alternatively, let's compute the original integral numerically using substitution. Let’s use substitution t = sqrt(x(2 -x)). Then, t ranges from 0 to1. But this might not help. Alternatively, use substitution θ as before. The integral became 2 ∫₀^{π/2} cos²θ cos(cosθ) dθ. Let's approximate this integral numerically. Let's use θ from 0 to π/2, and use a numerical method.

Let’s approximate ∫₀^{π/2} cos²θ cos(cosθ) dθ. Let's use Simpson's rule with n=4 intervals. The interval width h = (π/2)/4 ≈ 0.3927.

Compute the function at θ=0, h, 2h, 3h, 4h:

θ=0: cos²0 cos(cos0) = 1 * cos(1) ≈ 1 * 0.5403023059 ≈ 0.5403023059

θ=0.3927: cos²(0.3927) cos(cos(0.3927)). Compute cos(0.3927) ≈ cos(0.3927) ≈ 0.9231. Then cos²(0.3927) ≈ (0.9231)^2 ≈ 0.8521. cos(0.9231) ≈ 0.6045. So product ≈ 0.8521 * 0.6045 ≈ 0.5150.

θ=0.7854 (π/4): cos²(π/4) = (sqrt(2)/2)^2 = 0.5. cos(cos(π/4)) = cos(sqrt(2)/2) ≈ cos(0.7071) ≈ 0.7602. Product ≈ 0.5 * 0.7602 ≈ 0.3801.

θ=1.1781 (3h): cos²(1.1781) ≈ cos²(1.1781) ≈ (cos(1.1781))^2. cos(1.1781) ≈ 0.3827, so squared ≈ 0.1465. cos(0.3827) ≈ 0.9272. Product ≈ 0.1465 * 0.9272 ≈ 0.1358.

θ=1.5708 (π/2): cos²(π/2) = 0. cos(cos(π/2)) = cos(0) =1. Product=0.

Now, apply Simpson's rule:

Integral ≈ (h/3) [f0 + 4f1 + 2f2 +4f3 + f4]

= (0.3927/3) [0.5403 + 4*0.5150 + 2*0.3801 +4*0.1358 +0] ]

Calculate the terms inside:

0.5403 + 4*0.5150 = 0.5403 + 2.06 = 2.6003

2*0.3801 = 0.7602

4*0.1358 = 0.5432

Total: 2.6003 +0.7602 +0.5432 = 3.9037

Multiply by 0.3927/3 ≈ 0.1309 * 3.9037 ≈ 0.5105

Multiply by 2 (since the original integral is 2 times this): 2 * 0.5105 ≈ 1.0210

Which is close to the previous result of approximately 1.021657. So, this suggests that the exact answer is indeed (π/2)( J₀(1) - J₂(1) ), and the numerical approximation is approximately 1.021657382, which rounds to 1.0216573820 to 10 decimal places.

Therefore, the exact answer is (π/2)( J₀(1) - J₂(1) ), and the numerical approximation is approximately 1.0216573820.
</think>

{"answer": "\\frac{\\pi}{2} \\left(J_0(1) - J_2(1)\\right)", "numerical_answer": "1.0216573820"}