Let
\[
I = \int_0^1 \frac{x^2}{\sqrt{1+x^2}} \ln\left(x+\sqrt{1+x^2}\right) \arccos x\, dx
\]

We'll proceed step by step.

---

**Step 1: Use substitution**

Let us consider the substitution:
\[
x = \sin\theta,\quad dx = \cos\theta\, d\theta,\quad x \in [0,1] \implies \theta \in [0, \frac{\pi}{2}]
\]
Compute all relevant expressions in terms of \(\theta\):

- \(x^2 = \sin^2\theta\)
- \(1 + x^2 = 1 + \sin^2\theta = 1 + \sin^2\theta\)
- \(\sqrt{1 + x^2} = \sqrt{1 + \sin^2\theta}\)
- \(x + \sqrt{1 + x^2} = \sin\theta + \sqrt{1 + \sin^2\theta}\)
- \(\arccos x = \arccos(\sin\theta) = \frac{\pi}{2} - \theta\)

So,
\[
I = \int_0^{\pi/2}
\frac{\sin^2\theta}{\sqrt{1 + \sin^2\theta}}
\ln\left(\sin\theta+\sqrt{1+\sin^2\theta}\right)
\left(\frac{\pi}{2}-\theta\right)
\cos\theta\, d\theta
\]

---

**Step 2: Simplify with symmetry and integrate by parts**

Let \(u = \frac{\pi}{2} - \theta\), \(du = -d\theta\), as \(\theta\) goes from \(0\) to \(\pi/2\), \(u\) goes from \(\frac{\pi}{2}\) to \(0\).

Alternatively, consider expanding the integrand. Let us attempt integration by parts.

Let
\[
u = \arccos x, \quad dv = \frac{x^2}{\sqrt{1+x^2}} \ln(x + \sqrt{1+x^2}) dx
\]
then,
\(
du = -\frac{1}{\sqrt{1-x^2}} dx
\)

Let us compute \(v\):

Let us let \(A(x) = \frac{x^2}{\sqrt{1+x^2}} \ln(x + \sqrt{1+x^2})\).

But integrating this directly is challenging. Instead, let's try another substitution.

Let us try hyperbolic substitution:

Let \(x = \sinh t\), so \(x \in [0, 1] \Rightarrow t \in [0, \sinh^{-1} 1]\).

Compute:

- \(x = \sinh t\)
- \(dx = \cosh t\, dt\)
- \(x^2 = \sinh^2 t\)
- \(\sqrt{1+x^2} = \sqrt{1 + \sinh^2 t} = \cosh t\)
- \(x + \sqrt{1+x^2} = \sinh t + \cosh t = e^t\)
- \(\ln(x + \sqrt{1+x^2}) = \ln(e^t) = t\)
- \(\arccos x = \arccos(\sinh t)\)

Therefore,
\[
I = \int_{t=0}^{t_1}
\frac{\sinh^2 t}{\cosh t} \cdot t \cdot \arccos(\sinh t) \cdot \cosh t\, dt
\]
But \(\cosh t\) in denominator cancels with numerator:
\[
\frac{\sinh^2 t}{\cosh t} \cdot \cosh t = \sinh^2 t
\]
So,
\[
I = \int_{t=0}^{t_1} \sinh^2 t \cdot t \cdot \arccos(\sinh t) dt
\]
where \(t_1 = \sinh^{-1} 1 = \ln(1 + \sqrt{2})\).

Also, for \(t \in [0, \sinh^{-1} 1]\), \(\sinh t \in [0, 1]\) which matches the domain of the original arccos function.

---

**Step 3: Express arccos(\(\sinh t\)) in terms of t**

Set \(z = \sinh t\), so \(\arccos z\).

Alternatively, let's see if we can relate \(\arccos(\sinh t)\) to t.

Let \(z = \sinh t\), so \(t = \operatorname{arcsinh} z\), \(z \in [0,1]\).

\[
\cos \theta = x \to \theta = \arccos x
\]
But with \(x = \sinh t\), \(\theta = \arccos(\sinh t)\).

But for now, let's keep it at

\[
I = \int_{t=0}^{\ln(1+\sqrt{2})} \sinh^2 t \cdot t \cdot \arccos(\sinh t)\, dt
\]

Now, let's try integrating by parts with:

Let \(u = \arccos(\sinh t)\), \(dv = \sinh^2 t \cdot t dt\)

Then:
\[
du = \frac{d}{dt} \arccos(\sinh t)\, dt = -\frac{1}{\sqrt{1 - (\sinh t)^2}} \cosh t\, dt \]

But
\[
1 - \sinh^2 t = \cosh^2 t - \sinh^2 t = 1
\implies \sqrt{1 - (\sinh t)^2} = \sqrt{1 - \sinh^2 t} = \sqrt{\cosh^2 t - \sinh^2 t} = \sqrt{1}
= 1 \qquad ???
\]
Wait, that's not quite right, because \(1 - \sinh^2 t = \cosh^2 t - \sinh^2 t = 1\).

But originally, \(\arccos(\sinh t)\) is only defined for \(\sinh t \in [-1,1]\), i.e. \(t \in [-\sinh^{-1}(1), \sinh^{-1}(1)]\). Indeed, for \(t \in [0,\ln(1+\sqrt{2})]\), \(\sinh t \in [0,1]\).

But then
\[
\frac{d}{dt} \arccos(\sinh t) = -\frac{\cosh t}{\sqrt{1 - \sinh^2 t}}
= -\frac{\cosh t}{\sqrt{\cos^2h t - \sinh^2 t}} = -\frac{\cosh t}{\sqrt{1}}
= -\cosh t
\]

Therefore,
\[
du = -\cosh t dt
\]

Let \(v = \int \sinh^2 t \cdot t\, dt\).

Let us compute \(v\):

First, \(\sinh^2 t = \frac{1}{2} (\cosh 2t - 1)\).

Thus,

\[
\sinh^2 t \cdot t = \frac{1}{2} t\, (\cosh 2t - 1)
= \frac{1}{2} t\cosh 2t - \frac{1}{2} t
\]

Compute \(\int t \cosh 2t\, dt\):

Let us recall \(\int t \cosh(at)\, dt = \frac{1}{a} t \sinh(at) - \frac{1}{a^2} \cosh(at)\).

For \(a=2\):

\[
\int t \cosh 2t dt = \frac{1}{2} t \sinh 2t - \frac{1}{4} \cosh 2t
\]

Thus,

\[
v = \frac{1}{2} \left[ \frac{1}{2} t \sinh 2t - \frac{1}{4} \cosh 2t \right] - \frac{1}{2} \int t\, dt
= \frac{1}{4} t \sinh 2t - \frac{1}{8} \cosh 2t - \frac{1}{4} t^2
\]

Therefore,
\[
v = \frac{1}{4} t \sinh 2t - \frac{1}{8} \cosh 2t - \frac{1}{4} t^2
\]

---

**Step 4: Integration by parts**

Recall,

\[
I = \int u \, dv = uv \Big|_a^b - \int v\, du
\]

Therefore,

\[
I = \left. \arccos(\sinh t) \left( \frac{1}{4} t \sinh 2t - \frac{1}{8} \cosh 2t - \frac{1}{4} t^2 \right) \right|_{t=0}^{t_1}
+ \int_{0}^{t_1} \left( \frac{1}{4} t \sinh 2t - \frac{1}{8} \cosh 2t - \frac{1}{4} t^2 \right) \cosh t\, dt
\]

where \(t_1 = \ln(1+\sqrt{2})\).

Let me clarify: the derivative \(du\) is \(-\cosh t dt\), so the sign of the integral above flips:

\[
I = \left. \arccos(\sinh t) v \right|_0^{t_1} + \int_{0}^{t_1} v \cdot \cosh t dt
\]
As \(du = -\cosh t dt\), so:

\[
I = \left[ \arccos(\sinh t)\ v \right]_0^{t_1} + \int_0^{t_1} v \cdot \cosh t dt
\]

Let's write \(v\) as above.

So the next step is to compute
\[
J = \int_0^{t_1} \left( \frac{1}{4} t \sinh 2t - \frac{1}{8} \cosh 2t - \frac{1}{4} t^2 \right) \cosh t dt
\]

Let's expand this term by term.

---

**Step 5: Compute definite values in the boundary term**

Recall,

- \(t_1 = \ln(1 + \sqrt{2})\)
- At \(t=0\): \(\sinh 0 = 0\), \(\arccos(0) = \frac{\pi}{2}\)
- At \(t=t_1\): \(\sinh t_1 = 1\), \(\arccos(1) = 0\)

So,

At \(t=0\):

- \(\arccos(\sinh 0) = \arccos(0) = \frac{\pi}{2}\)
- \(t = 0, \sinh 2t = 0\), \(\cosh 2t = 1\), \(t^2 = 0\)

So, \(v(0) = \frac{1}{4} \cdot 0 \cdot 0 - \frac{1}{8} \cdot 1 - \frac{1}{4}\cdot 0 = -\frac{1}{8}\)

At \(t_1\):

- \(\arccos(\sinh t_1) = \arccos(1) = 0\)
- So the entire boundary term vanishes at \(t_1\).

Thus,
\[
\text{Boundary term: } \left. \arccos(\sinh t) v \right|_0^{t_1} = 0 - \left( \frac{\pi}{2} \cdot \left[ -\frac{1}{8} \right] \right) = \frac{\pi}{16}
\]

---

**Step 6: Compute the integral term**

Now, expand:
\[
J = \int_0^{t_1} \left( \frac{1}{4} t \sinh 2t - \frac{1}{8} \cosh 2t - \frac{1}{4} t^2 \right) \cosh t dt
\]

Let's compute each separately.

(a) First term: \(\int t \sinh 2t\, \cosh t dt\)

Express \(\sinh 2t\) using the double angle:
\[
\sinh 2t = 2 \sinh t \cosh t
\]
So:
\[
t \sinh 2t \cosh t = 2 t \sinh t (\cosh t)^2
\]

Thus,

\[
\int_0^{t_1} t \sinh 2t \cosh t dt
= 2 \int_0^{t_1} t \sinh t (\cosh t)^2 dt
\]

Now, \((\cosh t)^2 = \frac{1}{2} (\cosh 2t + 1)\), so:

\[
(\cosh t)^2 = \frac{1}{2} \cosh 2t + \frac{1}{2}
\]

Thus,
\[
t \sinh t (\cosh t)^2
= t \sinh t \left(\frac{1}{2} \cosh 2t + \frac{1}{2}\right)
= \frac{1}{2} t \sinh t \cosh 2t + \frac{1}{2} t \sinh t
\]

Therefore,
\[
\int_0^{t_1} t \sinh 2t \cosh t dt
= 2 \left[ \frac{1}{2} \int_0^{t_1} t \sinh t \cosh 2t dt + \frac{1}{2}\int_0^{t_1} t \sinh t dt \right]
= \int_0^{t_1} t \sinh t \cosh 2t dt + \int_0^{t_1} t \sinh t dt
\]

Let us evaluate these two terms.

---

**Compute \(\int t \sinh t dt\):**

Standard:
\[
\int t \sinh t dt = t \cosh t - \sinh t + C
\]

---

**Compute \(\int t \sinh t \cosh 2t dt\):**

Let’s use the identity:
\[
\sinh t \cosh 2t = \sinh t (2 \sinh t \cosh t) + \sinh t \cosh t
\]
Wait, let's compute \(\sinh t \cosh 2t\) directly:

\(\cosh 2t = 2 \cosh^2 t - 1\), so:

\[
\sinh t \cosh 2t = \sinh t (2 \cosh^2 t - 1) = 2 \sinh t \cosh^2 t - \sinh t
\]

But maybe it's better to write \(\sinh t \cosh 2t\) in terms of exponentials:
\[
\sinh t = \frac{e^{t} - e^{-t}}{2},\;
\cosh 2t = \frac{e^{2t} + e^{-2t}}{2}
\]
So,
\[
\sinh t \cosh 2t = \frac{e^{t} - e^{-t}}{2} \cdot \frac{e^{2t} + e^{-2t}}{2}
= \frac{1}{4} \left[ (e^{t} \cdot e^{2t}) + (e^{t} \cdot e^{-2t}) - (e^{-t} \cdot e^{2t}) - (e^{-t} \cdot e^{-2t}) \right]
= \frac{1}{4} [ e^{3t} + e^{-t} - e^{t} - e^{-3t} ]
\]

Therefore,
\[
t \sinh t \cosh 2t = \frac{1}{4} t (e^{3t} + e^{-t} - e^{t} - e^{-3t})
\]

So,
\[
\int t \sinh t \cosh 2t dt
= \frac{1}{4} \int t e^{3t} dt
+ \frac{1}{4} \int t e^{-t} dt
- \frac{1}{4} \int t e^{t} dt
- \frac{1}{4} \int t e^{-3t} dt
\]

Standard formula: \(\int t e^{a t} dt = \frac{e^{a t}}{a^2}(a t - 1)\)

Therefore,

- \(\int t e^{3t} dt = \frac{e^{3t}}{9}(3t - 1)\)
- \(\int t e^{-t} dt = \frac{e^{-t}}{1}( -t - 1) = - (t + 1) e^{-t}\)
- \(\int t e^{t} dt = e^{t} (t - 1)\)
- \(\int t e^{-3t} dt = \frac{e^{-3t}}{9}(-3t - 1)\)

Therefore,

\[
\int t \sinh t \cosh 2t dt = \frac{1}{4} \left[
\frac{e^{3t}}{9}(3t-1)
- (t+1) e^{-t}
- e^{t}(t-1)
- \frac{e^{-3t}}{9}(3t+1)
\right]
\]

Let’s expand:

\[
= \frac{1}{12} e^{3t}(t - \frac{1}{3}) - \frac{1}{4} (t+1) e^{-t}
- \frac{1}{4} e^{t}(t-1)
- \frac{1}{12} e^{-3t}(t + \frac{1}{3})
\]

---

So, returning to the term:

The first term in \(J\):
\[
\frac{1}{4} \int_0^{t_1} t \sinh 2t \cosh t dt
\]
But from above, we found:
\[
\int_0^{t_1} t \sinh 2t \cosh t dt = \int_0^{t_1} t \sinh t \cosh 2t dt + \int_0^{t_1} t \sinh t dt
\]
So, we can compute:

- \(\int_0^{t_1} t \sinh t \cosh 2t dt\): as above.
- \(\int_0^{t_1} t \sinh t dt\):

\[
\int t \sinh t dt = t \cosh t - \sinh t
\]

---

**Second term**: \(-\frac{1}{8} \int_0^{t_1} \cosh 2t \cosh t dt\)

\[
\cosh 2t \cosh t = \frac{1}{2}[\cosh(3t) + \cosh t]
\]
Therefore,
\[
-\frac{1}{8} \int_0^{t_1} \cosh 2t \cosh t dt
= -\frac{1}{16} \int_0^{t_1} \cosh 3t dt - \frac{1}{16} \int_0^{t_1} \cosh t dt
\]
\[
\int \cosh a t dt = \frac{1}{a} \sinh a t
\]
Therefore,
\[
\int_0^{t_1} \cosh 3t dt = \frac{1}{3}[\sinh 3t_1 - 0 ]
\]
\[
\int_0^{t_1} \cosh t dt = \sinh t_1
\]
Therefore,
\[
-\frac{1}{8} \int_0^{t_1} \cosh 2t \cosh t dt =
-\frac{1}{16} \cdot \frac{1}{3} \sinh 3t_1 - \frac{1}{16} \sinh t_1
\]

---

**Third term**: \(-\frac{1}{4} \int_0^{t_1} t^2 \cosh t dt\)

We can integrate by parts:
Let \(u = t^2\), \(dv = \cosh t dt\)

\[
du = 2t dt,\quad v = \sinh t
\]
\[
\int t^2 \cosh t dt = t^2 \sinh t - \int 2 t \sinh t dt
\]

Also,
\[
\int t \sinh t dt = t \cosh t - \int \cosh t dt = t \cosh t - \sinh t
\]
So,
\[
\int 2 t \sinh t dt = 2 t \cosh t - 2 \sinh t
\]

Therefore,
\[
\int t^2 \cosh t dt = t^2 \sinh t - 2 t \cosh t + 2 \sinh t
\]

Thus,
\[
-\frac{1}{4} \int_0^{t_1} t^2 \cosh t dt = -\frac{1}{4}\left[
(t_1^2 \sinh t_1 - 2 t_1 \cosh t_1 + 2 \sinh t_1) - (0 - 0 + 0)
\right]
\]

---

**Step 7: Compile the results**

Let us summarize all terms:

\[
I = \frac{\pi}{16}
+ \frac{1}{4} \left( [F(t_1) - F(0)] + [G(t_1) - G(0)] \right)
- \frac{1}{16} \sinh 3 t_1
- \frac{1}{16} \sinh t_1
- \frac{1}{4} ( t_1^2 \sinh t_1 - 2 t_1 \cosh t_1 + 2 \sinh t_1 )
\]

Where

- \(F(t) = \int t \sinh t \cosh 2t dt\) (already computed explicitly above)
- \(G(t) = \int t \sinh t dt = t \cosh t - \sinh t\)

And from our previous calculation:
\[
\int t \sinh t \cosh 2t dt = \frac{1}{12} e^{3t}\left( t - \frac{1}{3} \right)
- \frac{1}{4} (t+1) e^{-t}
- \frac{1}{4} e^{t}(t-1)
- \frac{1}{12} e^{-3t} (t + \frac{1}{3})
\]

Therefore, let's write everything together.

Set
- \(t_1 = \ln(1+\sqrt{2})\)

Define:

\[
F_{\rm diff} = \left[
\frac{1}{12} e^{3t_1}(t_1 - \frac{1}{3})
- \frac{1}{4} (t_1+1) e^{-t_1}
- \frac{1}{4} e^{t_1}(t_1 - 1)
- \frac{1}{12} e^{-3t_1}(t_1 + \frac{1}{3})
\right]
- \left[
\frac{1}{12} e^{0}(0 - \frac{1}{3})
- \frac{1}{4} (0+1) e^{0}
- \frac{1}{4} e^{0}(0 - 1)
- \frac{1}{12} e^{0}(0 + \frac{1}{3})
\right]
\]
Evaluate at \(t = 0\):

\(
\frac{1}{12} (1) (-1/3) = -\frac{1}{36}
\)

\(
- \frac{1}{4}(1) = -\frac{1}{4}
\)

\(
-\frac{1}{4}(1)(-1) = \frac{1}{4}
\)

\(
-\frac{1}{12}\cdot 1\cdot (1/3) = -\frac{1}{36}
\)

So sum: \(-\frac{1}{36}-\frac{1}{4}+\frac{1}{4}-\frac{1}{36} = -\frac{1}{18}\)

Thus, the zero endpoint contributes \(-\frac{1}{18}\).

Let’s write everything cleaned up.

Let’s define

\[
I = \frac{\pi}{16} + \frac{1}{4} \left( X \right) - \frac{1}{16} \sinh 3 t_1 - \frac{1}{16} \sinh t_1 - \frac{1}{4} ( t_1^2 \sinh t_1 - 2 t_1 \cosh t_1 + 2 \sinh t_1 )
\]

where

\[
X = F(t_1) + G(t_1) + \frac{1}{18}
\]

with

\[
F(t_1) = \frac{1}{12} e^{3 t_1}(t_1 - \frac{1}{3})
- \frac{1}{4} (t_1+1) e^{-t_1}
- \frac{1}{4} e^{t_1}(t_1 - 1)
- \frac{1}{12} e^{-3 t_1}(t_1 + \frac{1}{3})
\]
and
\[
G(t_1) = t_1 \cosh t_1 - \sinh t_1
\]

---

**Step 8: Numerical evaluation**

Let’s compute all constants.

- \(t_1 = \ln(1+\sqrt{2}) \approx 0.8813735870\)
- \(e^{t_1} = 1+\sqrt{2} \approx 2.414213562\)
- \(e^{-t_1} \approx 0.4142135624\)
- \(e^{3 t_1} = (e^{t_1})^3 = (2.414213562)^3 \approx 14.08560155\)
- \(e^{-3 t_1} = (e^{-t_1})^3 \approx 0.07106781187\)
- \(\cosh t_1 = \frac{e^{t_1} + e^{-t_1}}{2} \approx (2.414213562 + 0.4142135624)/2 \approx 1.414213562\)
- \(\sinh t_1 = \frac{e^{t_1} - e^{-t_1}}{2} = (2.414213562 - 0.4142135624)/2 \approx 1.000000000\)

Let’s compute step by step.

First,

- \(t_1 = 0.8813735870\)
- \(t_1^2 = 0.7760455688\)
- \(e^{t_1} = 2.414213562\)
- \(e^{-t_1} = 0.4142135624\)
- \(e^{3 t_1} = 14.08560155\)
- \(e^{-3 t_1} = 0.07106781187\)
- \(\cosh t_1 = 1.414213562\)
- \(\sinh t_1 = 1.000000000\)
- \(\sinh 3 t_1 = ?\)
- \(\sinh t_1 = 1\)

Compute \(F(t_1):\)

\[
F(t_1) =
\frac{1}{12} \cdot 14.08560155 \cdot (0.8813735870 - 0.3333333333)
- \frac{1}{4} \cdot (0.8813735870 + 1) \cdot 0.4142135624
- \frac{1}{4} \cdot 2.414213562 \cdot (0.8813735870 - 1)
- \frac{1}{12} \cdot 0.07106781187 \cdot (0.8813735870 + 0.3333333333)
\]

Compute each term:

- \(0.8813735870 - 0.3333333333 = 0.5480402537\)
- First term: \(14.08560155 \cdot 0.5480402537 = 7.724166679\), then divided by 12: \(0.6436805566\)
- \(0.8813735870 + 1 = 1.881373587\)
- Second term: \(1.881373587 \cdot 0.4142135624 = 0.7795162582\), then divided by 4: \(0.1948790645\) (so negative: \(-0.1948790645\))
- \(0.8813735870 - 1 = -0.1186264130\), \(2.414213562 \cdot -0.1186264130 = -0.2865418709\), divided by 4: \(-0.0716354677\), negative: \(+0.0716354677\)
- \(0.8813735870 + 0.3333333333 = 1.214706920\)
- \(0.07106781187 \cdot 1.214706920 = 0.08635420984\), divided by 12: \(0.007196184153\) (negative): \(-0.007196184153\)

Sum:

- \(0.6436805566 - 0.1948790645 + 0.0716354677 - 0.007196184153 =\)
- \(0.6436805566 - 0.1948790645 = 0.4488014921\)
- \(+ 0.0716354677 = 0.5204369598\)
- \(- 0.0071961842 = 0.5132407757\)

Thus, \(F(t_1) \approx 0.5132407757\)

Now, \(G(t_1) = t_1 \cosh t_1 - \sinh t_1 = 0.8813735870 \cdot 1.414213562 - 1.0 = 1.246340724 - 1 = 0.2463407242\)

Add \(F(t_1) + G(t_1) = 0.5132407757 + 0.2463407242 = 0.7595814999\)

Now add \(1/18 \approx 0.05555555556\)

So \(X = 0.7595814999 + 0.05555555556 = 0.8151370555\)

Then, \(Y = \frac{1}{4} X = 0.2037842639\)

---

Now compute the other terms:

- \(\sinh t_1 = 1\)
- \(\sinh 3 t_1 = ?\)

Let us compute \(3 t_1 = 2.644120761\)
\[
\sinh(2.644120761) = \frac{ e^{2.644120761} - e^{-2.644120761} }{2 }
\]
\(e^{2.644120761} \approx \exp(2.644120761) = 14.08560155\)
\(e^{-2.644120761} \approx 0.07106781187\)

\[
\sinh 3 t_1 = \frac{14.08560155 - 0.07106781187}{2} = \frac{14.01453374}{2} = 7.007266870
\]
Now, \(\frac{1}{16} \sinh 3 t_1 = 0.4380041794\)

And, \(\frac{1}{16} \sinh t_1 = 0.0625\)

And, \(\frac{1}{4} ( t_1^2 \sinh t_1 - 2 t_1 \cosh t_1 + 2 \sinh t_1 ) \):

First, \(t_1^2 \sinh t_1 = 0.7760455688 \cdot 1 = 0.7760455688\)
\(2 t_1 \cosh t_1 = 2 \cdot 0.8813735870 \cdot 1.414213562 = 2 \cdot 1.246340724 = 2.492681449\)
\(2 \sinh t_1 = 2 \cdot 1 = 2\)

Now,
\(0.7760455688 - 2.492681449 + 2 = 0.7760455688 + 2 - 2.492681449 = 2.776045569 - 2.492681449 = 0.2833641199\)

So,
\(\frac{1}{4} \cdot 0.2833641199 = 0.07084103\)

Now, total sum:

\[
I = \frac{\pi}{16} + 0.2037842639 - 0.4380041794 - 0.0625 - 0.07084103
\]
But be careful with the signs:
- \(-\frac{1}{16} \sinh 3 t_1 = -0.4380041794\)
- \(-\frac{1}{16} \sinh t_1 = -0.0625\)
- \(-\frac{1}{4} (\ldots) = -0.07084103\)

Now, \(\frac{\pi}{16} \approx 0.1963495408\)

So,

Sum all:

- \(0.1963495408\)
- \(+ 0.2037842639\)
- \(= 0.4001338047\)
- \(- 0.4380041794 = -0.0378703747\)
- \(- 0.0625 = -0.1003703747\)
- \(- 0.07084103 = -0.1712114047\)

Therefore, to 10 decimal places,
\[
I \approx -0.1712114047
\]

---

### **Final Step: Formatting the result**

**Exact answer in LaTeX:**

\[
\boxed{
I = \frac{\pi}{16} + \frac{1}{4} \left( F(t_1) + G(t_1) + \frac{1}{18} \right)
- \frac{1}{16} \sinh 3 t_1
- \frac{1}{16} \sinh t_1
- \frac{1}{4} ( t_1^2 \sinh t_1 - 2 t_1 \cosh t_1 + 2 \sinh t_1 )
}
\]
where
\[
t_1 = \ln(1+\sqrt{2})
\]
\[
F(t_1) = \frac{1}{12} e^{3 t_1}(t_1 - \frac{1}{3})
- \frac{1}{4} (t_1+1) e^{-t_1}
- \frac{1}{4} e^{t_1}(t_1 - 1)
- \frac{1}{12} e^{-3 t_1}(t_1 + \frac{1}{3})
\]
\[
G(t_1) = t_1 \cosh t_1 - \sinh t_1
\]

You may also write:

\[
\begin{align*}
I ={} & \frac{\pi}{16}
+ \frac{1}{4} \left[
\frac{1}{12} e^{3t_1}(t_1 - \frac{1}{3})
- \frac{1}{4} (t_1+1) e^{-t_1}
- \frac{1}{4} e^{t_1}(t_1 - 1)
- \frac{1}{12} e^{-3 t_1}(t_1 + \frac{1}{3}) \right. \\
& \left. + t_1 \cosh t_1 - \sinh t_1 + \frac{1}{18}
\right]
- \frac{1}{16} \sinh 3 t_1
- \frac{1}{16} \sinh t_1
- \frac{1}{4} ( t_1^2 \sinh t_1 - 2 t_1 \cosh t_1 + 2 \sinh t_1 )
\end{align*}
\]
where \(t_1 = \ln(1+\sqrt{2})\).

And numerically (rounded to 10 decimals):

\[
I \approx -0.1712114047
\]

---

### **Final JSON answer:**

```json
{"answer": "\\frac{\\pi}{16} + \\frac{1}{4} \\left[ \\frac{1}{12} e^{3 t_1}(t_1 - \\frac{1}{3}) - \\frac{1}{4} (t_1+1) e^{-t_1} - \\frac{1}{4} e^{t_1}(t_1 - 1) - \\frac{1}{12} e^{-3 t_1}(t_1 + \\frac{1}{3}) + t_1 \\cosh t_1 - \\sinh t_1 + \\frac{1}{18} \\right ] \\\\ - \\frac{1}{16} \\sinh 3 t_1 - \\frac{1}{16} \\sinh t_1 - \\frac{1}{4} ( t_1^2 \\sinh t_1 - 2 t_1 \\cosh t_1 + 2 \\sinh t_1 ),\\quad t_1 = \\ln(1+\\sqrt{2})", "numerical_answer": "-0.1712114047"}
```