We need to evaluate

  I = ∫ from -1/2 to 1/2  (1/(1 - x²)) dx.

Step 1. Write the integrand in partial fractions. Notice that
  1/(1 - x²) = 1/((1 - x)(1 + x)).
It can be decomposed as
  1/(1 - x²) = ½[1/(1 - x) + 1/(1 + x)].

Step 2. Find the antiderivative.
Integrate term by term:
  ∫[1/(1 - x)] dx = -ln|1 - x| + C,
  ∫[1/(1 + x)] dx = ln|1 + x| + C.
Thus,
  ∫ (1/(1 - x²)) dx = ½[ -ln|1 - x| + ln|1 + x| ] + C
            = ½ ln |(1 + x)/(1 - x)| + C.

Step 3. Evaluate the definite integral from x = -½ to x = ½.
Compute the antiderivative at the bounds:
 At x = ½:
  F(½) = ½ ln((1 + ½)/(1 - ½)) = ½ ln((3/2)/(1/2)) = ½ ln(3).
 At x = -½:
  F(-½) = ½ ln((1 - ½)/(1 + ½)) = ½ ln((1/2)/(3/2)) = ½ ln(1/3) = -½ ln(3).
Then, the definite integral I is:
  I = F(½) - F(-½) = ½ ln(3) - (-½ ln(3)) = ln(3).

Step 4. Provide a numerical approximation.
The natural logarithm of 3 is approximately:
  ln(3) ≈ 1.0986122887 (rounded to 10 decimal places).

Thus, the final answer in the required JSON format is:
{"answer": "\\ln(3)", "numerical_answer": "1.0986122887"}