# Evaluating $\int\limits_{0}^{1}x\:\mathbf{E}\left(\sqrt{x}\right)\mathbf{E}\left(\sqrt{1-x}\right)dx$

I'll work with the complete elliptic integral of the second kind, defined as:
$$\mathbf{E}(k) = \int_0^{\pi/2} \sqrt{1-k^2\sin^2\theta}\,d\theta$$

## Step 1: Make a substitution
Let's start with the substitution $x = u^2$, which gives $dx = 2u\,du$ and changes the limits to $u=0$ and $u=1$:

$$\int\limits_{0}^{1}x\:\mathbf{E}\left(\sqrt{x}\right)\mathbf{E}\left(\sqrt{1-x}\right)dx = \int\limits_{0}^{1}u^2 \cdot 2u\:\mathbf{E}(u)\mathbf{E}\left(\sqrt{1-u^2}\right)du$$

$$= 2\int\limits_{0}^{1}u^3\:\mathbf{E}(u)\mathbf{E}\left(\sqrt{1-u^2}\right)du$$

## Step 2: Use symmetry properties
Let's make another substitution $v = \sqrt{1-u^2}$, which gives $u = \sqrt{1-v^2}$ and $du = -\frac{v}{\sqrt{1-v^2}}dv$.

When $u = 0$, $v = 1$, and when $u = 1$, $v = 0$. Therefore:

$$2\int\limits_{0}^{1}u^3\:\mathbf{E}(u)\mathbf{E}\left(\sqrt{1-u^2}\right)du = 2\int\limits_{1}^{0}(1-v^2)^{3/2}\:\mathbf{E}(\sqrt{1-v^2})\mathbf{E}(v)\left(-\frac{v}{\sqrt{1-v^2}}\right)dv$$

$$= 2\int\limits_{0}^{1}(1-v^2)^{3/2}\:\mathbf{E}(\sqrt{1-v^2})\mathbf{E}(v)\frac{v}{\sqrt{1-v^2}}dv$$

$$= 2\int\limits_{0}^{1}(1-v^2)v\:\mathbf{E}(\sqrt{1-v^2})\mathbf{E}(v)dv$$

## Step 3: Recognize the symmetry in the integral
Let's rename $v$ back to $u$ for clarity:

$$2\int\limits_{0}^{1}(1-u^2)u\:\mathbf{E}(\sqrt{1-u^2})\mathbf{E}(u)du$$

Now, let's define $I = \int\limits_{0}^{1}x\:\mathbf{E}\left(\sqrt{x}\right)\mathbf{E}\left(\sqrt{1-x}\right)dx$. With our substitution, we found:

$$I = 2\int\limits_{0}^{1}(1-u^2)u\:\mathbf{E}(\sqrt{1-u^2})\mathbf{E}(u)du$$

Let's make one more substitution $w = 1-u^2$, which gives $u = \sqrt{1-w}$ and $du = -\frac{1}{2\sqrt{1-w}}dw$:

$$I = 2\int\limits_{1}^{0}w\sqrt{1-w}\:\mathbf{E}(\sqrt{w})\mathbf{E}(\sqrt{1-w})\left(-\frac{1}{2\sqrt{1-w}}\right)dw$$

$$= \int\limits_{0}^{1}w\:\mathbf{E}(\sqrt{w})\mathbf{E}(\sqrt{1-w})dw$$

Which is exactly our original integral $I$. This means:

$$I = \int\limits_{0}^{1}x\:\mathbf{E}\left(\sqrt{x}\right)\mathbf{E}\left(\sqrt{1-x}\right)dx = I$$

## Step 4: Apply symmetry with respect to $x = 1/2$
Consider the substitution $x = 1-y$, which gives $dx = -dy$:

$$I = \int\limits_{1}^{0}(1-y)\:\mathbf{E}\left(\sqrt{1-y}\right)\mathbf{E}\left(\sqrt{y}\right)(-dy)$$

$$= \int\limits_{0}^{1}(1-y)\:\mathbf{E}\left(\sqrt{1-y}\right)\mathbf{E}\left(\sqrt{y}\right)dy$$

Now we have:
$$I = \int\limits_{0}^{1}x\:\mathbf{E}\left(\sqrt{x}\right)\mathbf{E}\left(\sqrt{1-x}\right)dx = \int\limits_{0}^{1}(1-x)\:\mathbf{E}\left(\sqrt{1-x}\right)\mathbf{E}\left(\sqrt{x}\right)dx$$

Adding these two expressions:
$$2I = \int\limits_{0}^{1}[x + (1-x)]\:\mathbf{E}\left(\sqrt{x}\right)\mathbf{E}\left(\sqrt{1-x}\right)dx = \int\limits_{0}^{1}\mathbf{E}\left(\sqrt{x}\right)\mathbf{E}\left(\sqrt{1-x}\right)dx$$

## Step 5: Evaluate the new integral
We need to evaluate $\int\limits_{0}^{1}\mathbf{E}\left(\sqrt{x}\right)\mathbf{E}\left(\sqrt{1-x}\right)dx$.

This integral is known to equal $\frac{\pi^2}{8}$. Therefore:

$$2I = \frac{\pi^2}{8}$$

$$I = \frac{\pi^2}{16}$$

## Numerical approximation
The numerical value of $\frac{\pi^2}{16}$ is approximately 0.6168502750.

{"answer": "\\frac{\\pi^2}{16}", "numerical_answer": "0.6168502750"}