
To solve the definite integral \(\int_0^1\left(\frac{x^2}{2-x^2}+\sqrt{\frac{2x}{x+1}}\right)\:dx\), we split it into two parts and evaluate each separately.

### Part 1: \(I_1 = \int_0^1 \frac{x^2}{2-x^2}\,dx\)
Rewrite the integrand by decomposing the fraction:
\[
\frac{x^2}{2-x^2} = -1 + \frac{2}{2-x^2}
\]
Thus,
\[
I_1 = \int_0^1 \left(-1 + \frac{2}{2-x^2}\right) dx = \int_0^1 -1\,dx + 2\int_0^1 \frac{1}{2-x^2}\,dx
\]
The first integral is straightforward:
\[
\int_0^1 -1\,dx = -[x]_0^1 = -1
\]
For the second integral, use the standard result \(\int \frac{1}{a^2 - x^2}\,dx = \frac{1}{2a}\ln\left|\frac{a+x}{a-x}\right| + C\) with \(a = \sqrt{2}\):
\[
2\int_0^1 \frac{1}{2-x^2}\,dx = 2 \cdot \frac{1}{2\sqrt{2}} \left[\ln\left(\frac{\sqrt{2}+x}{\sqrt{2}-x}\right)\right]_0^1 = \frac{1}{\sqrt{2}} \left[\ln\left(\frac{\sqrt{2}+1}{\sqrt{2}-1}\right) - \ln(1)\right]
\]
Simplify \(\frac{\sqrt{2}+1}{\sqrt{2}-1} = (\sqrt{2}+1)^2 = 3 + 2\sqrt{2}\), so:
\[
2\int_0^1 \frac{1}{2-x^2}\,dx = \frac{1}{\sqrt{2}} \ln(3 + 2\sqrt{2})
\]
Thus,
\[
I_1 = -1 + \frac{1}{\sqrt{2}} \ln(3 + 2\sqrt{2})
\]

### Part 2: \(I_2 = \int_0^1 \sqrt{\frac{2x}{x+1}}\,dx\)
Use the substitution \(t = \sqrt{\frac{2x}{x+1}}\), which implies \(t^2 = \frac{2x}{x+1}\). Solving for \(x\) gives \(x = \frac{t^2}{2 - t^2}\), and \(dx = \frac{4t}{(2 - t^2)^2}dt\). The limits change from \(x=0 \to t=0\) to \(x=1 \to t=1\). The integral becomes:
\[
I_2 = \int_0^1 t \cdot \frac{4t}{(2 - t^2)^2} dt = \int_0^1 \frac{4t^2}{(2 - t^2)^2} dt
\]
Decompose the integrand:
\[
\frac{4t^2}{(2 - t^2)^2} = \frac{8}{(2 - t^2)^2} - \frac{4}{2 - t^2}
\]
Integrate term by term. For \(\int \frac{8}{(2 - t^2)^2}dt\), use the standard result \(\int \frac{1}{(a^2 - x^2)^2}dx = \frac{x}{2a^2(a^2 - x^2)} + \frac{1}{4a^3}\ln\left|\frac{a+x}{a-x}\right| + C\) with \(a = \sqrt{2}\):
\[
\int \frac{8}{(2 - t^2)^2}dt = \frac{2t}{2 - t^2} + \frac{1}{\sqrt{2}} \ln\left(\frac{\sqrt{2}+t}{\sqrt{2}-t}\right)
\]
For \(\int \frac{4}{2 - t^2}dt\), use the same standard result as before:
\[
\int \frac{4}{2 - t^2}dt = \sqrt{2} \ln\left(\frac{\sqrt{2}+t}{\sqrt{2}-t}\right)
\]
Combining these and evaluating from \(0\) to \(1\):
\[
I_2 = \left[\frac{2t}{2 - t^2} + \frac{1}{\sqrt{2}} \ln\left(\frac{\sqrt{2}+t}{\sqrt{2}-t}\right) - \sqrt{2} \ln\left(\frac{\sqrt{2}+t}{\sqrt{2}-t}\right)\right]_0^1
\]
Simplify using \(\ln(3 + 2\sqrt{2}) = 2\ln(\sqrt{2}+1)\) and evaluating at the limits gives:
\[
I_2 = 2 - \sqrt{2} \ln(\sqrt{2} + 1)
\]

### Total Integral
Adding \(I_1\) and \(I_2\):
\[
I_1 + I_2 = \left(-1 + \frac{1}{\sqrt{2}} \ln(3 + 2\sqrt{2})\right) + \left(2 - \sqrt{2} \ln(\sqrt{2} + 1)\right)
\]
Since \(\frac{1}{\sqrt{2}} \ln(3 + 2\sqrt{2}) = \sqrt{2} \ln(\sqrt{2} + 1)\), the logarithmic terms cancel, leaving:
\[
I_1 + I_2 = 1
\]

### Numerical Approximation
The exact value is \(1\), so the numerical approximation is \(1.0000000000\).

{"answer": "1", "numerical_answer": "1.0000000000"}