We begin with the integral

  I = ∫₀¹ √[4]{(1/x) – 1} dx = ∫₀¹ (1/x – 1)^(1/4) dx.

Step 1. Make the substitution

  u⁴ = 1/x – 1  ⟹  1/x = u⁴ + 1  ⟹  x = 1/(u⁴ + 1).

Differentiate x with respect to u:
  dx/du = –4u³/(u⁴ + 1)²  ⟹  dx = –4u³/(u⁴ + 1)² du.

Note the limits. When x = 1,
  1/x – 1 = 0  ⟹  u = 0.
When x → 0⁺,
  1/x → ∞  ⟹  u⁴ → ∞  ⟹  u → ∞.

Also, using our substitution, the integrand simplifies:
  √[4]{1/x – 1} = u.

Thus, the integral becomes

  I = ∫_(x=0)^(x=1) u · [dx] = ∫_(u=∞)^(u=0) u · (–4u³/(u⁴ + 1)² du)
     = 4 ∫₀^∞ u⁴/(u⁴ + 1)² du.

Step 2. Write the integrand in a more convenient form:
  u⁴/(u⁴ + 1)² = [ (u⁴ + 1) – 1 ]/(u⁴ + 1)² = 1/(u⁴ + 1) – 1/(u⁴ + 1)².
Thus,
  I = 4 [ ∫₀^∞ 1/(u⁴ + 1) du – ∫₀^∞ 1/(u⁴ + 1)² du ].

Step 3. Evaluation of the two integrals.
A known result is
  ∫₀^∞ du/(1+u⁴) = π/(2√2).

For the second integral, we use a standard Beta-integral formula:
  ∫₀∞ u^(m–1)/(1+uⁿ)ᵖ du = (1/n) B(m/n, p – m/n),
valid when the parameters are in the proper range. Here, set m = 1 (so that u^(0)=1), n = 4, and p = 2. Then
  ∫₀∞ du/(1+u⁴)² = (1/4) B(1/4, 2 – 1/4) = (1/4) B(1/4, 7/4)
     = (1/4) [Γ(1/4) Γ(7/4)]/Γ(2).
Since Γ(2) = 1, we have
  ∫₀∞ 1/(1+u⁴)² du = (1/4) Γ(1/4) Γ(7/4).

Thus,
  I = 4 [ π/(2√2) – (1/4) Γ(1/4)Γ(7/4) ]
     = 2π/√2 – Γ(1/4)Γ(7/4)
     = π√2 – Γ(1/4)Γ(7/4).

Step 4. Simplify the Gamma product.
Using the recurrence relation, note that
  Γ(7/4) = (3/4) Γ(3/4).
A well-known formula is
  Γ(1/4) Γ(3/4) = π√2.
Thus,
  Γ(1/4) Γ(7/4) = (3/4)[Γ(1/4)Γ(3/4)] = (3/4)(π√2) = 3π√2/4.

Substitute back:
  I = π√2 – (3π√2/4) = π√2 (1 – 3/4) = (π√2)/4.

Step 5. Numerical Approximation.
Compute:
  π ≈ 3.1415926536,
  √2 ≈ 1.4142135624,
so
  (π√2)/4 ≈ (3.1415926536 × 1.4142135624) / 4 ≈ 4.4428829382/4 ≈ 1.1107207345.

Thus, the exact answer is (π√2)/4 and the numerical approximation is 1.1107207345.

{"answer": "\\frac{\\pi\\sqrt{2}}{4}", "numerical_answer": "1.1107207345"}