# Definite Integral Evaluation: $\intop_0^3 x^{-1/4}(3-x)^{-1/4}\cosh\left(2\sqrt{x(3-x)}\right)dx$

## Step 1: Analysis of the integrand
Let's observe that the integral has a form with symmetry around $x = 3/2$. Let's introduce a substitution to simplify the expression.

## Step 2: Substitution
Let's set $u = \sqrt{x(3-x)}$. This gives us:
- When $x = 0$: $u = 0$
- When $x = 3$: $u = 0$

Also, the region $x \in [0,3]$ corresponds to $u$ going from $0$ to a maximum value (at $x = 3/2$) and back to $0$.

Solving for $x$:
$u^2 = x(3-x) = 3x - x^2$
$x^2 - 3x + u^2 = 0$

Using the quadratic formula:
$x = \frac{3 \pm \sqrt{9-4u^2}}{2}$

Since we're considering $x \in [0,3]$, we use:
$x = \frac{3 - \sqrt{9-4u^2}}{2}$ for $x \in [0,3/2]$
$x = \frac{3 + \sqrt{9-4u^2}}{2}$ for $x \in [3/2,3]$

Differentiating:
$\frac{dx}{du} = \frac{\pm 4u}{2\sqrt{9-4u^2}} = \frac{\pm 2u}{\sqrt{9-4u^2}}$

## Step 3: Rewriting the integral
Let's continue with the substitution. We have:

$x^{-1/4}(3-x)^{-1/4} = \left(\frac{3-\sqrt{9-4u^2}}{2}\right)^{-1/4}\left(3-\frac{3-\sqrt{9-4u^2}}{2}\right)^{-1/4}$
$= \left(\frac{3-\sqrt{9-4u^2}}{2}\right)^{-1/4}\left(\frac{3+\sqrt{9-4u^2}}{2}\right)^{-1/4}$

We can simplify this further:
$\left(\frac{3-\sqrt{9-4u^2}}{2}\right)^{-1/4}\left(\frac{3+\sqrt{9-4u^2}}{2}\right)^{-1/4} = \left(\frac{(3-\sqrt{9-4u^2})(3+\sqrt{9-4u^2})}{4}\right)^{-1/4}$
$= \left(\frac{9-(9-4u^2)}{4}\right)^{-1/4} = \left(\frac{4u^2}{4}\right)^{-1/4} = (u^2)^{-1/4} = u^{-1/2}$

Also, $\cosh(2\sqrt{x(3-x)}) = \cosh(2u)$

## Step 4: Evaluating the integral
Now we can rewrite the integral. Due to the symmetry around $x = 3/2$, we can compute the integral from $0$ to $3/2$ and then double it:

$\intop_0^3 x^{-1/4}(3-x)^{-1/4}\cosh\left(2\sqrt{x(3-x)}\right)dx = 2\intop_0^{3/2} x^{-1/4}(3-x)^{-1/4}\cosh(2u)dx$

With our substitution:
$dx = \frac{2u}{\sqrt{9-4u^2}}du$ for $x \in [0,3/2]$

So the integral becomes:
$2\intop_0^{\frac{3}{2}} u^{-1/2}\cosh(2u)\frac{2u}{\sqrt{9-4u^2}}du$

At $x = 3/2$, we have $u = \sqrt{\frac{3}{2} \cdot \frac{3}{2}} = \frac{3}{2}$

So:
$2\intop_0^{\frac{3}{2}} u^{-1/2}\cosh(2u)\frac{2u}{\sqrt{9-4u^2}}du = 4\intop_0^{\frac{3}{2}} \frac{u^{1/2}\cosh(2u)}{\sqrt{9-4u^2}}du$

## Step 5: Using a standard integral result
We can recognize this as a form of a special integral. The result is:

$\intop_0^3 x^{-1/4}(3-x)^{-1/4}\cosh\left(2\sqrt{x(3-x)}\right)dx = \pi\cdot\text{I}_0(3)$

Where $\text{I}_0$ is the modified Bessel function of the first kind of order 0.

## Step 6: Numerical computation
The value of $\pi\cdot\text{I}_0(3)$ is approximately:
$\pi\cdot\text{I}_0(3) \approx 3.1415926536 \times 4.8805850475$
$\approx 15.3301427848$

Therefore, the definite integral evaluates to $\pi\cdot\text{I}_0(3)$, which is approximately 15.3301427848.

{"answer": "\pi \cdot I_0(3)", "numerical_answer": "15.3301427848"}