

To solve the definite integral \(\int_{0}^{2} x^{-1/2} (2-x)^{-1/2} [1-0.5x(2-x)] \, dx\), we proceed as follows:

### Step 1: Simplify the Integrand
First, expand the term inside the brackets:
\[
1 - 0.5x(2 - x) = 1 - x + 0.5x^2
\]
Thus, the integrand becomes:
\[
x^{-1/2}(2 - x)^{-1/2}(1 - x + 0.5x^2)
\]

### Step 2: Substitution to Beta Function Form
Use the substitution \(t = \frac{x}{2}\), so \(x = 2t\) and \(dx = 2dt\). When \(x = 0\), \(t = 0\); when \(x = 2\), \(t = 1\). Substituting:
- \(x^{-1/2} = (2t)^{-1/2} = 2^{-1/2}t^{-1/2}\)
- \((2 - x)^{-1/2} = [2(1 - t)]^{-1/2} = 2^{-1/2}(1 - t)^{-1/2}\)
- \(1 - 0.5x(2 - x) = 1 - 2t(1 - t) = 1 - 2t + 2t^2\)

The integrand transforms to:
\[
\left(2^{-1/2}t^{-1/2}\right)\left(2^{-1/2}(1 - t)^{-1/2}\right)(1 - 2t + 2t^2) \cdot 2dt = t^{-1/2}(1 - t)^{-1/2}(1 - 2t + 2t^2)dt
\]
Thus, the integral becomes:
\[
\int_{0}^{1} t^{-1/2}(1 - t)^{-1/2}(1 - 2t + 2t^2) \, dt
\]

### Step 3: Split into Beta Functions
The integral splits into three terms:
\[
\int_{0}^{1} t^{-1/2}(1 - t)^{-1/2} \, dt - 2\int_{0}^{1} t^{1/2}(1 - t)^{-1/2} \, dt + 2\int_{0}^{1} t^{3/2}(1 - t)^{-1/2} \, dt
\]
These are beta functions \(B(a, b) = \int_{0}^{1} t^{a-1}(1 - t)^{b-1} \, dt = \frac{\Gamma(a)\Gamma(b)}{\Gamma(a+b)}\), where \(\Gamma\) is the gamma function.

### Step 4: Evaluate Each Beta Function
1. First term: \(B\left(\frac{1}{2}, \frac{1}{2}\right) = \frac{\Gamma\left(\frac{1}{2}\right)\Gamma\left(\frac{1}{2}\right)}{\Gamma(1)} = \frac{(\sqrt{\pi})(\sqrt{\pi})}{1} = \pi\)
2. Second term: \(B\left(\frac{3}{2}, \frac{1}{2}\right) = \frac{\Gamma\left(\frac{3}{2}\right)\Gamma\left(\frac{1}{2}\right)}{\Gamma(2)} = \frac{\left(\frac{1}{2}\sqrt{\pi}\right)(\sqrt{\pi})}{1} = \frac{\pi}{2}\)
3. Third term: \(B\left(\frac{5}{2}, \frac{1}{2}\right) = \frac{\Gamma\left(\frac{5}{2}\right)\Gamma\left(\frac{1}{2}\right)}{\Gamma(3)} = \frac{\left(\frac{3}{4}\sqrt{\pi}\right)(\sqrt{\pi})}{2} = \frac{3\pi}{8}\)

### Step 5: Combine Results
\[
\pi - 2\left(\frac{\pi}{2}\right) + 2\left(\frac{3\pi}{8}\right) = \pi - \pi + \frac{3\pi}{4} = \frac{3\pi}{4}
\]

### Numerical Approximation
The numerical value of \(\frac{3\pi}{4}\) is approximately \(2.3561944902\) (rounded to 10 decimal places).

{"answer": "\\frac{3\\pi}{4}", "numerical_answer": "2.3561944902"}