

To solve the definite integral \( \int_{-1}^1 \frac{\cos x}{1 + e^{-\frac{1}{x}}} \, dx \), we proceed as follows:

### Step 1: Substitution for Symmetry
Let \( I = \int_{-1}^1 \frac{\cos x}{1 + e^{-\frac{1}{x}}} \, dx \). We use the substitution \( x = -t \), which transforms the integral:
- When \( x = -1 \), \( t = 1 \); when \( x = 1 \), \( t = -1 \).
- \( dx = -dt \), and \( \cos(-t) = \cos(t) \).

Thus,
\[
I = \int_{1}^{-1} \frac{\cos(-t)}{1 + e^{-\frac{1}{-t}}} (-dt) = \int_{-1}^1 \frac{\cos t}{1 + e^{\frac{1}{t}}} \, dt.
\]
Renaming \( t \) back to \( x \), we have:
\[
I = \int_{-1}^1 \frac{\cos x}{1 + e^{\frac{1}{x}}} \, dx.
\]

### Step 2: Adding the Original and Substituted Integrals
Add the original integral \( I \) and the substituted integral \( I \):
\[
2I = \int_{-1}^1 \left( \frac{\cos x}{1 + e^{-\frac{1}{x}}} + \frac{\cos x}{1 + e^{\frac{1}{x}}} \right) dx.
\]

### Step 3: Simplifying the Integrand
Simplify the integrand by combining the fractions. Let \( a = e^{\frac{1}{x}} \). Then \( e^{-\frac{1}{x}} = \frac{1}{a} \), so:
\[
\frac{1}{1 + e^{-\frac{1}{x}}} + \frac{1}{1 + e^{\frac{1}{x}}} = \frac{1}{1 + \frac{1}{a}} + \frac{1}{1 + a} = \frac{a}{a + 1} + \frac{1}{a + 1} = 1.
\]
Thus, the integrand simplifies to \( \cos x \), and:
\[
2I = \int_{-1}^1 \cos x \, dx.
\]

### Step 4: Evaluating the Integral
The integral of \( \cos x \) is \( \sin x \). Evaluating over \([-1, 1]\):
\[
\int_{-1}^1 \cos x \, dx = \sin(1) - \sin(-1) = \sin(1) + \sin(1) = 2\sin(1).
\]
Thus, \( 2I = 2\sin(1) \), so \( I = \sin(1) \).

### Numerical Approximation
The numerical value of \( \sin(1) \) (in radians) is approximately \( 0.8414709848 \) when rounded to 10 decimal places.

{"answer": "\(\sin(1)\)", "numerical_answer": "0.8414709848"}