Given the integral:

\[
I = \int\limits_{0}^{2} \frac{x^{-1/2}(2-x)^{-1/2}}{\sqrt{1 + x(2-x)}} T_3\left(\sqrt{1 + x(2-x)}\right) \, dx
\]

Where \(T_3(y)\) denotes the Chebyshev polynomial of degree 3:
\[
T_3(y) = 4y^3 - 3y
\]

Let's solve step by step.

---

### Step 1: Substitute \(x = 2 \sin^2 \theta\)

Let 
\[
x = 2 \sin^2 \theta, \quad dx = 4 \sin\theta \cos\theta\, d\theta
\]
As \(x\) goes from \(0\) to \(2\), \(\theta\) goes from \(0\) to \(\pi/2\).

Now calculate each term:
- \(x^{-1/2} = (2\sin^2\theta)^{-1/2} = \frac{1}{\sqrt{2}\sin\theta}\)
- \((2-x)^{-1/2} = (2-2\sin^2\theta)^{-1/2} = (2\cos^2\theta)^{-1/2} = \frac{1}{\sqrt{2}\cos\theta}\)
- \(x(2-x) = 2\sin^2\theta \cdot 2\cos^2\theta = 4\sin^2\theta\cos^2\theta = \sin^2 2\theta\)
- \(1 + x(2-x) = 1 + \sin^2 2\theta\)
- \(\sqrt{1 + x(2-x)} = \sqrt{1 + \sin^2 2\theta}\)

Now plug these into the integrand:

\[
I = \int_{0}^{\pi/2} 
\frac{\frac{1}{\sqrt{2}\sin\theta} \cdot \frac{1}{\sqrt{2}\cos\theta}}{\sqrt{1+\sin^2 2\theta}}
T_3\left(\sqrt{1 + \sin^2 2\theta}\right)
4 \sin\theta \cos\theta \, d\theta
\]

\[
= \int_0^{\pi/2} \frac{4 \cdot \sin\theta \cos\theta}{2 \sin\theta \cos\theta \sqrt{1+\sin^2 2\theta}} T_3\left(\sqrt{1 + \sin^2 2\theta}\right) d\theta
\]
\[
= \int_0^{\pi/2} \frac{2}{\sqrt{1+\sin^2 2\theta}} T_3\left(\sqrt{1 + \sin^2 2\theta}\right) d\theta
\]

---

### Step 2: Substitute the Chebyshev polynomial

Recall: \(T_3(y) = 4y^3 - 3y\), with \(y = \sqrt{1+\sin^2 2\theta}\):

\[
T_3\left(\sqrt{1+\sin^2 2\theta}\right) = 4 (1+\sin^2 2\theta)^{3/2} - 3 (1+\sin^2 2\theta)^{1/2}
\]

Thus,
\[
I = 2 \int_0^{\pi/2} 
\frac{4 (1+\sin^2 2\theta)^{3/2} - 3 (1+\sin^2 2\theta)^{1/2}}{\sqrt{1+\sin^2 2\theta}} d\theta
\]
\[
= 2 \int_0^{\pi/2} \left[ 4(1+\sin^2 2\theta) - 3 \right] d\theta
\]
\[
= 2 \int_0^{\pi/2} \left[ 4(1+\sin^2 2\theta) - 3 \right] d\theta
\]
\[
= 2 \int_0^{\pi/2} \left(4 + 4\sin^2 2\theta - 3\right) d\theta
\]
\[
= 2 \int_0^{\pi/2} \left(1 + 4 \sin^2 2\theta\right) d\theta
\]
\[
= 2 \int_0^{\pi/2} d\theta + 8 \int_0^{\pi/2} \sin^2 2\theta \, d\theta
\]
\[
= 2\left[ \theta \Big|_0^{\pi/2} \right] + 8\left[ \int_0^{\pi/2} \sin^2 2\theta \, d\theta \right]
\]
\[
= 2 \cdot \frac{\pi}{2} + 8 I_1, \quad \text{where } I_1 = \int_0^{\pi/2} \sin^2 2\theta \, d\theta
\]
\[
= \pi + 8I_1
\]

---

### Step 3: Evaluate \(\int_0^{\pi/2} \sin^2 2\theta \, d\theta\)

Recall:
\[
\sin^2 2\theta = \frac{1 - \cos 4\theta}{2}
\]

So,
\[
I_1 = \int_0^{\pi/2} \frac{1 - \cos 4\theta}{2} d\theta = \frac{1}{2}\int_0^{\pi/2} d\theta - \frac{1}{2}\int_0^{\pi/2}\cos 4\theta d\theta
\]
\[
= \frac{1}{2}\left[\theta\right]_0^{\pi/2} - \frac{1}{2}\left[\frac{\sin 4\theta}{4}\right]_0^{\pi/2}
\]
\[
= \frac{1}{2}\left( \frac{\pi}{2} \right) - \frac{1}{2} \cdot \frac{1}{4} \left( \sin 4 \cdot \frac{\pi}{2} - \sin 0 \right )
\]
\[
= \frac{\pi}{4} - \frac{1}{8} ( \sin 2\pi - 0 )
\]
\[
\sin 2\pi = 0 \implies I_1 = \frac{\pi}{4}
\]

---

### Step 4: Plug Back and Find Answer

\[
I = \pi + 8 \cdot \frac{\pi}{4} = \pi + 2\pi = 3\pi
\]

---

### Step 5: Numerical Approximation

\[
3\pi \approx 3 \times 3.1415926536 = 9.4247779608
\]

---

### Step 6: JSON Output

```json
{"answer": "3\\pi", "numerical_answer": "9.4247779608"}
```