Let's compute the definite integral
\[
I = \int_{\frac{1}{8}}^{\frac{1}{4}} \frac{\ln(2x)\ln(4x)\ln(8x)}{x} \, dx
\]

### 1. Simplification

Letâ€™s first write \(\ln(2x)\), \(\ln(4x)\), and \(\ln(8x)\) in terms of \(\ln x\):

- \(\ln(2x) = \ln 2 + \ln x\)
- \(\ln(4x) = \ln 4 + \ln x = 2\ln 2 + \ln x\)
- \(\ln(8x) = \ln 8 + \ln x = 3\ln 2 + \ln x\)

Therefore, the product is:
\[
(\ln 2 + \ln x)(2\ln 2 + \ln x)(3\ln 2 + \ln x)
\]

Let \(y = \ln x\) and \(L = \ln 2\), then:
\[
(\ln 2 + y)(2\ln 2 + y)(3\ln 2 + y) = \prod_{k=1}^3 (kL + y)
\]

Expand carefully:

First, expand two factors:
\[
(\ln 2 + y)(2\ln 2 + y) = (L + y)(2L + y) = 2L^2 + 3L y + y^2
\]

Multiply by the third factor:
\[
[2L^2 + 3L y + y^2] (3L + y) \\
= 2L^2 (3L + y) + 3L y (3L + y) + y^2 (3L + y)
\]

Compute each:
- \(2L^2 (3L + y) = 6L^3 + 2L^2 y\)
- \(3L y (3L + y) = 9L^2 y + 3L y^2\)
- \(y^2(3L + y) = 3L y^2 + y^3\)

Total:
- \(L^3\) : \(6\)
- \(L^2 y\) : \(2 + 9 = 11\)
- \(L y^2\) : \(3 + 3 = 6\)
- \(y^3\) : \(1\)

So:
\[
(\ln 2 + y)(2\ln 2 + y)(3\ln 2 + y) = 6L^3 + 11L^2 y + 6L y^2 + y^3
\]
with \(L = \ln 2\).

So the integral is:
\[
I = \int_{x=1/8}^{1/4} \frac{6L^3 + 11L^2 \ln x + 6L (\ln x)^2 + (\ln x)^3}{x} dx
\]

### 2. Integrate Term by Term

Each term can be integrated as:

- \(\int \frac{dx}{x} = \ln x\)
- \(\int \frac{(\ln x)^n}{x} dx = \frac{(\ln x)^{n+1}}{n+1}\)

So:

\[
I = 6L^3 \int_{x=1/8}^{1/4} \frac{dx}{x} +
    11L^2 \int_{x=1/8}^{1/4} \frac{\ln x}{x} dx +
    6L \int_{x=1/8}^{1/4} \frac{(\ln x)^2}{x} dx +
    \int_{x=1/8}^{1/4} \frac{(\ln x)^3}{x} dx
\]

\[
= 6L^3 [\ln x]_{1/8}^{1/4}
+ 11L^2 \left[\frac{(\ln x)^2}{2}\right]_{1/8}^{1/4}
+ 6L \left[\frac{(\ln x)^3}{3}\right]_{1/8}^{1/4}
+ \left[\frac{(\ln x)^4}{4}\right]_{1/8}^{1/4}
\]

Arrange:
\[
I = 6L^3 \Delta_1
+ \frac{11}{2} L^2 \Delta_2
+ 2L \Delta_3
+ \frac{1}{4} \Delta_4
\]
where:
- \(\Delta_1 = \ln\left(\frac{1}{4}\right) - \ln\left(\frac{1}{8}\right) = \ln\left(\frac{1/4}{1/8}\right) = \ln 2\)
- \(\Delta_2 = (\ln(\frac{1}{4}))^2 - (\ln(\frac{1}{8}))^2\)
- \(\Delta_3 = (\ln(\frac{1}{4}))^3 - (\ln(\frac{1}{8}))^3\)
- \(\Delta_4 = (\ln(\frac{1}{4}))^4 - (\ln(\frac{1}{8}))^4\)

Calculate logarithms:

- \(\ln(1/4) = \ln 1 - \ln 4 = 0 - 2\ln 2 = -2L\)
- \(\ln(1/8) = 0 - 3\ln 2 = -3L\)

So:

- \(\Delta_1 = -2L - (-3L) = L\)
- \(\Delta_2 = (-2L)^2 - (-3L)^2 = 4L^2 - 9L^2 = -5L^2\)
- \(\Delta_3 = (-2L)^3 - (-3L)^3 = (-8L^3) - (-27L^3) = 19L^3\)
- \(\Delta_4 = [(-2L)^4 - (-3L)^4] = [16L^4 - 81L^4] = -65L^4\)

Put all together:
\[
I = 6L^3 (L)
+ \frac{11}{2}L^2 (-5L^2)
+ 2L (19L^3)
+ \frac{1}{4}(-65L^4)
\]
\[
= 6L^4
- \frac{55}{2}L^4
+ 38L^4
- \frac{65}{4}L^4
\]

Sum up the coefficients:

- \(6 - \frac{55}{2} + 38 - \frac{65}{4}\)

Compute with common denominator (4):
- \(6 = 24/4\)
- \(-\frac{55}{2} = -110/4\)
- \(38 = 152/4\)
- \(-\frac{65}{4}\)

Sum:
\[
\frac{24 - 110 + 152 - 65}{4} = \frac{24 + 152}{4} - \frac{110 + 65}{4} = \frac{176}{4} - \frac{175}{4} = \frac{1}{4}
\]

So:

\[
I = \frac{1}{4}L^4 = \frac{1}{4}(\ln 2)^4
\]

### 3. Numerical Approximation

\(\ln 2 \approx 0.6931471806\)

\((\ln 2)^4 \approx (0.6931471806)^4 \approx\)
First, square it:
\((0.6931471806)^2 \approx 0.4808983469\)

Then square again:
\((0.4808983469)^2 \approx 0.2310490602\)

Thus,

\[
I = \frac{1}{4} \times 0.2310490602 \approx 0.05776226505
\]

### 4. JSON Output

```json
{"answer": "\\frac{1}{4}(\\ln 2)^4", "numerical_answer": "0.0577622651"}
```