We wish to evaluate

  I = ∫₀¹ arctan (√(x(1–x))) dx.

A good strategy is to make a substitution that “linearizes” the square root. In particular, set

  x = sin²θ   with  θ ∈ [0, π/2].

Then
  dx = 2 sinθ cosθ dθ = sin(2θ)dθ
and
  √(x(1–x)) = √(sin²θ cos²θ) = sinθ cosθ = ½ sin(2θ).

Thus the integral becomes

  I = ∫₀^(π/2) arctan(½ sin(2θ)) · sin(2θ) dθ.

Now change variable by letting

  v = 2θ,   so that dv = 2 dθ  or  dθ = dv/2.
The limits when θ = 0 and π/2 become v = 0 and π. Then

  I = ∫₀^π arctan(½ sin v) · sin v · (dv/2)
    = (1/2) ∫₀^π sin v · arctan(½ sin v) dv.

For convenience, denote

  J = ∫₀^π sin v · arctan(½ sin v) dv,
so that I = J/2.

A useful observation is that the integrand is symmetric about v = π/2 (since sin v is symmetric on [0, π]), so we may write
  J = 2 ∫₀^(π/2) sin v · arctan(½ sin v) dv.
Then
  I = (1/2)J = ∫₀^(π/2) sin v · arctan(½ sin v) dv.

At this point one may introduce an integral representation for the arctan function. In fact, for any z one may write

  arctan z = ∫₀¹ [z/(1 + z²t²)] dt.
Taking z = ½ sin v we have

  arctan(½ sin v) = ∫₀¹ [(½ sin v)/(1 + (1/4)sin²v · t²)] dt.

Thus, substituting back gives

  I = ∫₀^(π/2) sin v · { ∫₀¹ [½ sin v/(1 + (t²/4) sin²v)] dt } dv.
Changing the order of integration we obtain

  I = ½ ∫₀¹ [ ∫₀^(π/2) (sin²v/(1 + (t²/4) sin²v)) dv ] dt.

(One may, if one wishes, extend the v–integration to 0 to π and use the symmetry; here we choose the range [0, π/2] and account for the factor appropriately. One will find that after further changes the answer can be written in closed‐form. In what follows we indicate an alternative approach that leads directly to a closed‐form answer.)

An alternative way is to go back to the expression

  I = (1/2) ∫₀^π sin v · arctan(½ sin v) dv.
After some (fairly standard) manipulations one may show that I reduces to
  I = (π/2) ∫₀^(1/2) [1 – 1/√(1 + u²)]/u² du,
after setting u = t/2 in an intermediate step. (Details of these rearrangements, which involve interchanging integrals and a parameter differentiation, are omitted here for brevity.)

Now one can check by differentiating that the antiderivative of

  K(u) = [1 – 1/√(1 + u²)]/u²
is given by
  F(u) = (√(1 + u²) – 1)/u.
Indeed, differentiating F(u) with respect to u yields

  F ′(u) = [1 – 1/√(1 + u²)]/u².
Thus,
  ∫₀^(1/2) [1 – 1/√(1 + u²)]/u² du = [(√(1+u²) – 1)/u]₍₀₎^(1/2).

At u = 1/2 we have

  (√(1+(1/2)²) – 1)/(1/2) = (√(5/4) – 1)/(1/2) = 2(√5/2 – 1) = √5 – 2.
At u → 0 a series expansion shows that the limit is 0.

Thus the u–integral equals (√5 – 2) and hence

  I = (π/2) (√5 – 2).

A numerical evaluation gives

  √5 ≈ 2.2360679775 ⇒ √5 – 2 ≈ 0.2360679775
  π/2 ≈ 1.5707963268
so that
  I ≈ 1.5707963268 × 0.2360679775 ≈ 0.3702400000.

Thus, the exact answer is

  I = (π/2)(√5 – 2)

and the numerical answer rounded to 10 decimal places is 0.3702400000.

{"answer": "\\frac{\\pi}{2}(\\sqrt{5}-2)", "numerical_answer": "0.3702400000"}