To compute the definite integral \(\large\int_0^\infty\frac{\tanh(x)}{\exp(x)}dx\), we follow these steps:

### Step 1: Express \(\tanh(x)\) in terms of exponentials
Recall that:
\[
\tanh(x) = \frac{e^x - e^{-x}}{e^x + e^{-x}} = \frac{e^{2x} - 1}{e^{2x} + 1}
\]

### Step 2: Substitute \(\tanh(x)\) into the integral
The integral becomes:
\[
\int_0^\infty \frac{\tanh(x)}{e^x} dx = \int_0^\infty \frac{e^{2x} - 1}{e^{2x} + 1} \cdot e^{-x} dx = \int_0^\infty \frac{e^x - e^{-x}}{e^{2x} + 1} dx
\]

### Step 3: Simplify the integrand
Letâ€™s rewrite the integrand:
\[
\frac{e^x - e^{-x}}{e^{2x} + 1} = \frac{e^x}{e^{2x} + 1} - \frac{e^{-x}}{e^{2x} + 1}
\]

### Step 4: Split the integral
The integral splits into two parts:
\[
\int_0^\infty \frac{e^x}{e^{2x} + 1} dx - \int_0^\infty \frac{e^{-x}}{e^{2x} + 1} dx
\]

### Step 5: Evaluate the first integral \(\int_0^\infty \frac{e^x}{e^{2x} + 1} dx\)
Let \(u = e^x\), then \(du = e^x dx\). The limits change as follows:
- When \(x = 0\), \(u = 1\).
- When \(x = \infty\), \(u = \infty\).

The integral becomes:
\[
\int_1^\infty \frac{1}{u^2 + 1} du = \left. \arctan(u) \right|_1^\infty = \frac{\pi}{2} - \frac{\pi}{4} = \frac{\pi}{4}
\]

### Step 6: Evaluate the second integral \(\int_0^\infty \frac{e^{-x}}{e^{2x} + 1} dx\)
Let \(v = e^{-x}\), then \(dv = -e^{-x} dx\). The limits change as follows:
- When \(x = 0\), \(v = 1\).
- When \(x = \infty\), \(v = 0\).

The integral becomes:
\[
-\int_1^0 \frac{v}{v^{-2} + 1} dv = \int_0^1 \frac{v}{1 + v^{-2}} dv = \int_0^1 \frac{v^3}{1 + v^2} dv
\]

Simplify the integrand:
\[
\frac{v^3}{1 + v^2} = v - \frac{v}{1 + v^2}
\]

Thus:
\[
\int_0^1 \left(v - \frac{v}{1 + v^2}\right) dv = \left. \frac{v^2}{2} \right|_0^1 - \left. \frac{1}{2} \ln(1 + v^2) \right|_0^1 = \frac{1}{2} - \frac{1}{2} \ln(2)
\]

### Step 7: Combine the results
Subtract the second integral from the first:
\[
\frac{\pi}{4} - \left(\frac{1}{2} - \frac{1}{2} \ln(2)\right) = \frac{\pi}{4} - \frac{1}{2} + \frac{1}{2} \ln(2)
\]

### Step 8: Numerical approximation
Compute the numerical value:
\[
\frac{\pi}{4} \approx 0.7853981634, \quad \frac{1}{2} = 0.5, \quad \frac{1}{2} \ln(2) \approx 0.3465735903
\]
\[
0.7853981634 - 0.5 + 0.3465735903 \approx 0.6319717537
\]

### Final Answer
The exact answer is:
\[
\frac{\pi}{4} - \frac{1}{2} + \frac{1}{2} \ln(2)
\]
The numerical approximation is:
\[
0.6319717537
\]

### JSON Output
```json
{"answer": "\\frac{\\pi}{4} - \\frac{1}{2} + \\frac{1}{2} \\ln(2)", "numerical_answer": "0.6319717537"}
```