

To calculate the definite integral \(\int_0^\pi \cos(x + \cos(x)) \, dx\), we proceed as follows:

### Step 1: Expand the integrand using trigonometric identities
Using the cosine addition formula \(\cos(A + B) = \cos A \cos B - \sin A \sin B\), we rewrite the integrand:
\[
\cos(x + \cos(x)) = \cos(x)\cos(\cos(x)) - \sin(x)\sin(\cos(x)).
\]
Thus, the integral splits into two parts:
\[
\int_0^\pi \cos(x + \cos(x)) \, dx = \int_0^\pi \cos(x)\cos(\cos(x)) \, dx - \int_0^\pi \sin(x)\sin(\cos(x)) \, dx.
\]

### Step 2: Evaluate the second integral (\(I_2\))
Let \(I_2 = \int_0^\pi \sin(x)\sin(\cos(x)) \, dx\). Use the substitution \(u = \cos(x)\), so \(du = -\sin(x) \, dx\). When \(x = 0\), \(u = 1\); when \(x = \pi\), \(u = -1\). The integral becomes:
\[
I_2 = \int_{1}^{-1} \sin(u) \cdot (-du) = \int_{-1}^{1} \sin(u) \, du.
\]
Since \(\sin(u)\) is an odd function, \(\int_{-a}^{a} \sin(u) \, du = 0\). Thus, \(I_2 = 0\).

### Step 3: Evaluate the first integral (\(I_1\))
Let \(I_1 = \int_0^\pi \cos(x)\cos(\cos(x)) \, dx\). Use the substitution \(x = \pi - t\), so \(dx = -dt\). When \(x = 0\), \(t = \pi\); when \(x = \pi\), \(t = 0\). The integral becomes:
\[
I_1 = \int_{\pi}^{0} \cos(\pi - t)\cos(\cos(\pi - t)) \cdot (-dt) = \int_0^\pi -\cos(t)\cos(-\cos(t)) \, dt.
\]
Since \(\cos(-\cos(t)) = \cos(\cos(t))\) (cosine is even), this simplifies to:
\[
I_1 = -\int_0^\pi \cos(t)\cos(\cos(t)) \, dt = -I_1.
\]
Thus, \(I_1 = -I_1\), which implies \(I_1 = 0\).

### Step 4: Combine results
The original integral is \(I_1 - I_2 = 0 - 0 = 0\).

### Numerical Approximation
The exact value is \(0\), so the numerical approximation is \(0.0000000000\).

{"answer": "0", "numerical_answer": "0.0000000000"}