


To solve the definite integral \(\int_{0}^{1} x^{-1/4}(1 - x)^{-1/4}\cos\left(\sqrt{x(1 - x)}\right)dx\), we proceed as follows:

### Step 1: Analytic Approach
The integrand involves \(x^{-1/4}(1 - x)^{-1/4}\) and \(\cos\left(\sqrt{x(1 - x)}\right)\). We expand the cosine term using its Taylor series:
\[
\cos(z) = \sum_{n=0}^{\infty} \frac{(-1)^n z^{2n}}{(2n)!}
\]
Let \(z = \sqrt{x(1 - x)}\), so \(z^{2n} = (x(1 - x))^n\). Substituting this into the integral, we get:
\[
\int_{0}^{1} x^{-1/4}(1 - x)^{-1/4} \sum_{n=0}^{\infty} \frac{(-1)^n (x(1 - x))^n}{(2n)!} dx
\]
Interchanging the sum and integral (justified by uniform convergence), we rewrite the integral as:
\[
\sum_{n=0}^{\infty} \frac{(-1)^n}{(2n)!} \int_{0}^{1} x^{n - 1/4}(1 - x)^{n - 1/4} dx
\]
The integral inside is a Beta function:
\[
\int_{0}^{1} x^{a-1}(1 - x)^{b-1} dx = B(a, b) = \frac{\Gamma(a)\Gamma(b)}{\Gamma(a + b)}
\]
Here, \(a = n + 3/4\) and \(b = n + 3/4\), so:
\[
\int_{0}^{1} x^{n - 1/4}(1 - x)^{n - 1/4} dx = B\left(n + \frac{3}{4}, n + \frac{3}{4}\right) = \frac{\Gamma\left(n + \frac{3}{4}\right)^2}{\Gamma\left(2n + \frac{3}{2}\right)}
\]
Thus, the integral becomes:
\[
\sum_{n=0}^{\infty} \frac{(-1)^n \Gamma\left(n + \frac{3}{4}\right)^2}{(2n)! \Gamma\left(2n + \frac{3}{2}\right)}
\]

### Step 2: Numerical Approximation
To approximate the series, we compute the first few terms:
- For \(n=0\): \(\frac{\Gamma(3/4)^2}{\Gamma(3/2)} \approx 1.6943\)
- For \(n=1\): \(-\frac{\Gamma(7/4)^2}{2 \cdot \Gamma(7/2)} \approx -0.1275\)
- For \(n=2\): \(\frac{\Gamma(11/4)^2}{24 \cdot \Gamma(11/2)} \approx 0.0021\)
- Higher terms are negligible.

Summing these gives an approximation of \(1.5690\).

### Final Answer
The exact answer is the infinite series, and the numerical approximation is approximately \(1.5690\).

```json
{"answer": "\\sum_{n=0}^{\\infty} \\frac{(-1)^n \\Gamma\\left(n + \\frac{3}{4}\\right)^2}{(2n)! \\Gamma\\left(2n + \\frac{3}{2}\\right)}", "numerical_answer": "1.5690000000"}
```