We wish to compute

  I = ∫₀¹ (sin(log x) – log x)⁄(log² x) dx.

Step 1. Make a substitution.

Let u = log x. Then x = eᵘ and dx = eᵘ du. When x = 0, u → −∞ and when x = 1, u = 0. Thus the integral becomes

  I = ∫₋∞⁰ [sin u − u]⁄u² · eᵘ du.

Step 2. Change the variable to remove the “minus” sign.

Set u = –t (so that t = –u and du = –dt). When u = –∞, t → ∞; when u = 0, t = 0. Then

  I = ∫ₜ=∞⁰ [sin(–t) − (–t)]⁄(–t)² · e^(–t)(–dt).

Notice:
 • sin(–t) = – sin t,
 • (–t)² = t²,
 • The two minus signs (one in sin and one in dt) will be handled upon reversing the limits.

Thus, rewriting we get

  I = ∫₀∞ [– sin t + t]⁄t² · e^(–t) dt  
     = ∫₀∞ (t – sin t) e^(–t)⁄t² dt.

Step 3. Introduce a parameter to help evaluate the integral.

Define, for a real parameter a,

  F(a) = ∫₀¹ [sin(a log x) – a log x]⁄(log² x) dx.

In these terms our desired integral is I = F(1). Differentiate F(a) with respect to a:

  F′(a) = d/da ∫₀¹ [sin(a log x) – a log x]⁄(log² x) dx  
       = ∫₀¹ {cos(a log x)·log x – log x}⁄(log² x) dx  
       = ∫₀¹ [cos(a log x) – 1]⁄(log x) dx.

Now substitute u = log x (so that x = eᵘ, dx = eᵘ du) with u going from −∞ to 0:

  F′(a) = ∫₋∞⁰ [cos(a u) – 1]⁄u · eᵘ du.

Next, let t = –u (so that u = –t, du = –dt). Then t runs from 0 to ∞ and we have:

  F′(a) = ∫₀∞ [cos(–a t) – 1]⁄(–t) · e^(–t)(–dt)
       = ∫₀∞ [cos(a t) – 1]⁄t · e^(–t) dt.

Step 4. Recognize a standard integral.

A standard integral (which can be verified by differentiating with respect to the parameter) is

  ∫₀∞ [1 – cos(b t)] e^(–t)⁄t dt = ½ ln(1 + b²).

Thus, replacing b with a we find

  ∫₀∞ [cos(a t) – 1] e^(–t)⁄t dt = –½ ln(1 + a²).

So

  F′(a) = –½ ln(1 + a²).

Step 5. Integrate F′(a).

Since F(0) = ∫₀¹ [sin(0 · log x) – 0]⁄(log² x) dx = 0, we integrate from 0 to 1:

  F(1) = F(1) – F(0) = ∫₀¹ F′(a) da = –½ ∫₀¹ ln(1 + a²) da.

Thus, our task is now to compute

  J = ∫₀¹ ln(1 + a²) da.

Step 6. Evaluate the auxiliary integral J.

Integrate by parts:
 Let u = ln(1 + a²) ⇒ du = (2a/(1 + a²)) da,
 and dv = da    ⇒ v = a.
Then

  J = a ln(1 + a²) |₀¹ – ∫₀¹ a · (2a/(1 + a²)) da  
    = [1 · ln2 – 0] – 2∫₀¹ a²/(1 + a²) da.

Notice that

  a²/(1 + a²) = 1 – 1/(1 + a²).

Thus

  ∫₀¹ a²/(1 + a²) da = ∫₀¹ [1 – 1/(1 + a²)] da  
     = [a]₀¹ – [arctan(a)]₀¹  
     = 1 – (π/4).

So

  J = ln2 – 2[1 – (π/4)] = ln2 – 2 + (π/2).

Step 7. Write the final answer.

Returning to our original integral,

  I = F(1) = –½ J = –½(ln2 – 2 + π/2).

That is,

  I = 1 – (π/4) – (½ ln2).

Step 8. Provide a numerical approximation.

Compute:
 π/4 ≈ 3.1415926536/4 ≈ 0.7853981634,
 ½ ln2 ≈ 0.5 × 0.6931471806 ≈ 0.3465735903,
and
 1 – 0.7853981634 ≈ 0.2146018366. Then
 I ≈ 0.2146018366 – 0.3465735903 ≈ –0.1319717537.

Thus, the exact answer is

  I = 1 – (π/4) – (½ ln2),

and numerically I ≈ –0.1319717537.

{"answer": "1 - \\frac{\\pi}{4} - \\frac{1}{2}\\ln 2", "numerical_answer": "-0.1319717537"}