To solve the definite integral \(\int_1^{2011} \frac{\sqrt{x}}{\sqrt{2012 - x} + \sqrt{x}} \, dx\), we will follow the steps outlined.

### Step 1: Analytical Computation

First, let's simplify the integrand. Consider the integral:
\[ I = \int_1^{2011} \frac{\sqrt{x}}{\sqrt{2012 - x} + \sqrt{x}} \, dx. \]

We can use a symmetry argument to simplify this integral. Notice that if we make the substitution \( u = 2012 - x \), then \( du = -dx \) and the limits of integration change as follows:
- When \( x = 1 \), \( u = 2011 \).
- When \( x = 2011 \), \( u = 1 \).

Thus, the integral becomes:
\[ I = \int_{2011}^{1} \frac{\sqrt{2012 - u}}{\sqrt{u} + \sqrt{2012 - u}} (-du) = \int_1^{2011} \frac{\sqrt{2012 - u}}{\sqrt{u} + \sqrt{2012 - u}} \, du. \]

Now, let's denote this new integral as \( J \):
\[ J = \int_1^{2011} \frac{\sqrt{2012 - u}}{\sqrt{u} + \sqrt{2012 - u}} \, du. \]

Notice that \( I \) and \( J \) are essentially the same integral but with the roles of \( x \) and \( 2012 - x \) swapped. Therefore, we can write:
\[ I = J. \]

Adding \( I \) and \( J \) together, we get:
\[ I + J = \int_1^{2011} \frac{\sqrt{x}}{\sqrt{2012 - x} + \sqrt{x}} \, dx + \int_1^{2011} \frac{\sqrt{2012 - x}}{\sqrt{x} + \sqrt{2012 - x}} \, dx. \]

Since the integrands are complementary fractions, their sum is 1:
\[ I + J = \int_1^{2011} 1 \, dx = 2011 - 1 = 2010. \]

Since \( I = J \), we have:
\[ 2I = 2010 \implies I = \frac{2010}{2} = 1005. \]

### Step 2: Numerical Approximation

The exact answer is \( 1005 \). To provide a numerical approximation rounded to 10 decimal places, we simply write:
\[ 1005.0000000000. \]

### Step 3: JSON Output

Finally, we output the answer in the required JSON format:
```json
{"answer": "1005", "numerical_answer": "1005.0000000000"}
```