<think>
Okay, let's see. I need to compute the definite integral from 0 to π/2 of cos(x)/(2 - cos²x) dx. Hmm, first, I should think about how to approach this integral. The integrand is cos(x) divided by (2 minus cos squared x). Maybe a substitution would work here. Let me try to simplify the denominator first. 

The denominator is 2 - cos²x. I remember that 1 - cos²x is sin²x, but here it's 2 minus cos²x. Maybe I can rewrite that as 1 + (1 - cos²x) which is 1 + sin²x. So the denominator becomes 1 + sin²x. Wait, that might not help directly. Let me check: 2 - cos²x = 1 + (1 - cos²x) = 1 + sin²x. Yes, that's correct. So the integral becomes ∫ cosx / (1 + sin²x) dx from 0 to π/2. 

Hmm, that seems more manageable. Now, maybe substitution. Let me set u = sinx. Then du/dx = cosx, so du = cosx dx. That's perfect because the numerator is cosx dx. So substituting, the integral becomes ∫ du / (1 + u²) from u=0 (when x=0) to u=1 (when x=π/2). Wait, the integral of 1/(1 + u²) du is arctan(u) + C. So evaluating from 0 to 1, that would be arctan(1) - arctan(0). 

Arctan(1) is π/4 and arctan(0) is 0. So the integral should be π/4. Wait, that seems straightforward. But let me double-check my substitution steps. 

Original integral: u = sinx, du = cosx dx. When x=0, u=0; x=π/2, u=1. So the integral becomes ∫₀¹ du/(1 + u²) = [arctan(u)]₀¹ = π/4 - 0 = π/4. That seems correct. 

But wait, the original denominator was 2 - cos²x, which I rewrote as 1 + sin²x. Let me confirm that substitution again. 2 - cos²x = 2 - (1 - sin²x) = 1 + sin²x. Yes, that's right. So the substitution is valid. 

Therefore, the exact answer is π/4. Numerically, π is approximately 3.1415926536, so π/4 is about 0.7853981634. Rounded to 10 decimal places, that's 0.7853981634. 

Wait, but let me check if there's another way to solve this integral, just to confirm. Maybe using a different substitution. Let's see. Suppose I didn't notice the denominator could be done that way. Let's try another approach. 

Alternatively, maybe use substitution t = tan(x/2), which is the Weierstrass substitution. But that might complicate things. Let me try. Let t = tan(x/2), so dx = 2/(1 + t²) dt. Then cosx = (1 - t²)/(1 + t²). Let's substitute into the integral. The denominator becomes 2 - [(1 - t²)/(1 + t²)]². Let's compute that:

Denominator: 2 - (1 - 2t² + t⁴)/(1 + t²)². Let's combine terms:

2(1 + t²)² - (1 - 2t² + t⁴) all over (1 + t²)².

Expanding 2(1 + 2t² + t⁴) - (1 - 2t² + t⁴) = 2 + 4t² + 2t⁴ -1 + 2t² - t⁴ = 1 + 6t² + t⁴.

So denominator is (1 + 6t² + t⁴)/(1 + t²)². Then the integrand becomes [ (1 - t²)/(1 + t²) ] / [ (1 + 6t² + t⁴)/(1 + t²)² ] * [2/(1 + t²) dt]. Let's simplify step by step:

Multiply numerator and denominator:

Numerator: (1 - t²) * (1 + t²)² * 2/(1 + t²) = (1 - t²)(1 + t²) * 2 = 2(1 - t⁴)

Denominator: (1 + 6t² + t⁴)(1 + t²)

Wait, this seems more complicated. Maybe this substitution isn't the best approach here. Let me check if I made a mistake in the algebra. Alternatively, perhaps this method isn't the right path. Let me go back to the first substitution which gave a straightforward answer. 

Alternatively, maybe check with another substitution. Let me consider the original integral: ∫ cosx/(2 - cos²x) dx. Let me set u = sinx, then du = cosx dx. Wait, but then the denominator is 2 - (1 - u²) = 1 + u². So the integral becomes ∫ du/(1 + u²), which is arctan(u) + C. So from u=0 to u=1, which is arctan(1) - arctan(0) = π/4. So same result. 

Therefore, the exact answer is π/4. The numerical approximation is approximately 0.7853981634. 

Wait, just to be thorough, let me compute the integral numerically using another method. Let's approximate the integral using a simple method like the midpoint rule with a few intervals to check. For example, take x from 0 to π/2. Let's pick a few points. But maybe that's overkill. Alternatively, use a calculator to compute the integral numerically. But since I know that π/4 is approximately 0.7853981634, which is the value we have. 

Alternatively, if I use substitution t = cosx, then dt = -sinx dx. Wait, but the integrand is cosx/(2 - cos²x) dx. If I set t = cosx, then dt = -sinx dx. Hmm, but the integrand has cosx in the numerator. Let's see:

∫ cosx/(2 - t²) dx. But t = cosx, so dt = -sinx dx. Hmm, not sure if that helps. Let's try:

Express the integral as ∫ t/(2 - t²) * dx. But we need to express dx in terms of dt. Since dt = -sinx dx, so dx = -dt/sinx. But sinx = sqrt(1 - t²). So dx = -dt/sqrt(1 - t²). Therefore, the integral becomes ∫ t/(2 - t²) * (-dt)/sqrt(1 - t²). The limits when x=0, t=1; x=π/2, t=0. So reversing the limits, the integral becomes ∫ from t=1 to t=0 of t/(2 - t²) * (-dt)/sqrt(1 - t²) = ∫ from 0 to 1 of t/(2 - t²) * dt/sqrt(1 - t²). 

So the integral is ∫₀¹ t / [(2 - t²) sqrt(1 - t²)] dt. Hmm, this seems more complicated than the previous substitution. Maybe not helpful. So perhaps the first substitution is the correct way. 

Therefore, I think the exact answer is π/4, and the numerical approximation is approximately 0.7853981634. So the final answer should be as such.
</think>

{"answer": "\\frac{\\pi}{4}", "numerical_answer": 0.7853981634}