<think>
Okay, so I need to compute the definite integral from -1 to 1 of [sin(sqrt(x)) / (sinh(sqrt(x)) + sin(sqrt(x)))] dx. Hmm, let's start by understanding the integrand. The function involves sin and sinh of sqrt(x), which might complicate things. First, I should check if the integrand is even or odd because the limits are symmetric around zero. That might simplify the problem.

Wait, the variable substitution could help here. Let me consider substituting t = sqrt(x). But since x ranges from -1 to 1, I need to be careful with the square root of a negative number. Oh, right! The original integral is from -1 to 1, but sqrt(x) is only real for x ≥ 0. For x < 0, sqrt(x) would involve imaginary numbers. But the integrand has sin(sqrt(x)) and sinh(sqrt(x)). Let me check if the integrand is defined for x in [-1, 1].

Wait, sinh(z) is defined for complex z, but here x is real. If x is negative, sqrt(x) is imaginary, so let's write sqrt(x) = i*sqrt(|x|) for x < 0. Then sin(sqrt(x)) becomes sin(i*sqrt(|x|)) = i sinh(sqrt(|x|)), using the identity sin(iz) = i sinh(z). Similarly, sinh(sqrt(x)) for x < 0 would be sinh(i*sqrt(|x|)) = i sin(sqrt(|x|)), since sinh(iz) = i sin(z). Let's verify that.

So, for x < 0, let x = -a where a > 0. Then sqrt(x) = i*sqrt(a). Then:

sin(sqrt(x)) = sin(i*sqrt(a)) = i sinh(sqrt(a))

sinh(sqrt(x)) = sinh(i*sqrt(a)) = i sin(sqrt(a))

Therefore, the integrand for x < 0 becomes [i sinh(sqrt(a))] / [i sin(sqrt(a)) + i sinh(sqrt(a))] = [i sinh(sqrt(a))] / [i (sin(sqrt(a)) + sinh(sqrt(a)))] = sinh(sqrt(a)) / (sin(sqrt(a)) + sinh(sqrt(a))).

So the integrand for x < 0 is sinh(sqrt(|x|)) / (sin(sqrt(|x|)) + sinh(sqrt(|x|))). 

Now, notice that the original integrand for x > 0 is sin(sqrt(x)) / (sinh(sqrt(x)) + sin(sqrt(x))). So, for x in [-1, 0), the integrand is sinh(sqrt(|x|)) / (sin(sqrt(|x|)) + sinh(sqrt(|x|))), and for x in [0,1], it's sin(sqrt(x)) / (sinh(sqrt(x)) + sin(sqrt(x))).

Now, let's consider the substitution t = sqrt(|x|). But maybe a substitution that combines both parts. Let's split the integral into two parts: from -1 to 0 and from 0 to 1.

So, integral from -1 to 1 = integral from -1 to 0 + integral from 0 to 1.

Let me handle the integral from -1 to 0 first. Let x = -a, where a goes from 0 to 1. Then dx = -da. So the integral becomes:

∫_{a=1}^{0} [sinh(sqrt(a)) / (sin(sqrt(a)) + sinh(sqrt(a)))] (-da) = ∫_{0}^{1} [sinh(sqrt(a)) / (sin(sqrt(a)) + sinh(sqrt(a)))] da.

Similarly, the integral from 0 to 1 is ∫_{0}^{1} [sin(sqrt(x)) / (sinh(sqrt(x)) + sin(sqrt(x)))] dx.

So the total integral is the sum of these two:

∫_{0}^{1} [sinh(sqrt(a)) / (sin + sinh) ] da + ∫_{0}^{1} [sin / (sinh + sin) ] dx.

But notice that the two integrands are:

First integral: sinh(t) / (sin(t) + sinh(t)) where t = sqrt(a)

Second integral: sin(t) / (sinh(t) + sin(t)) where t = sqrt(x)

So if we let t = sqrt(a) in the first integral and t = sqrt(x) in the second, then both integrals would be over t from 0 to 1. Let's make that substitution.

For the first integral: a = t^2, da = 2t dt. So the first becomes ∫_{0}^{1} [sinh(t) / (sin(t) + sinh(t))] * 2t dt.

Similarly, the second integral: x = t^2, dx = 2t dt. So it becomes ∫_{0}^{1} [sin(t) / (sinh(t) + sin(t))] * 2t dt.

Therefore, the total integral is 2 ∫_{0}^{1} t [ sinh(t)/(sin(t) + sinh(t)) + sin(t)/(sinh(t) + sin(t)) ] dt.

But the terms inside the brackets add up to [sinh(t) + sin(t)] / [sinh(t) + sin(t)] = 1. So the integrand simplifies to 2 ∫_{0}^{1} t * 1 dt = 2 * [ (1/2) t^2 ] from 0 to 1 = 2*(1/2 - 0) = 1.

Wait, that's a surprising simplification. So the integral from -1 to 1 is equal to 1? Let me check that again.

So, after splitting the integral into two parts and substituting variables, we found that each part contributes an integral over t from 0 to 1 of 2t times their respective fractions. But when we add the fractions, they sum to 1. Therefore, the entire integral becomes 2 ∫_{0}^{1} t * 1 dt = 2*(1/2) = 1. So the exact answer is 1.

But let me verify this step-by-step again to make sure I didn't make a mistake.

Original integral: ∫_{-1}^1 [sin(sqrt(x)) / (sinh(sqrt(x)) + sin(sqrt(x)))] dx.

Split into ∫_{-1}^0 and ∫_{0}^1.

For ∫_{-1}^0: substitute x = -a, dx = -da. Then integral becomes ∫_{1}^{0} [sinh(sqrt(a))/(sin(sqrt(a)) + sinh(sqrt(a)))] (-da) = ∫_{0}^{1 [sinh(sqrt(a))/(sin + sinh)] da.

Then, for both integrals, substitute t = sqrt(a) in the first and t = sqrt(x) in the second. Then, a = t^2, da = 2t dt, so first integral becomes ∫_{0}^{1} [sinh(t)/(sin(t) + sinh(t))] * 2t dt.

Similarly, the second integral becomes ∫_{0}^{1} [sin(t)/(sinh(t) + sin(t))] * 2t dt.

Adding them together: 2 ∫_{0}^{1} t [ sinh(t) + sin(t) ] / [ sinh(t) + sin(t) ] dt = 2 ∫_{0}^{1} t dt = 2*(1/2) = 1.

Yes, that seems correct. The key insight was recognizing that the integrand for negative values of x transforms into a complementary fraction that, when added to the positive part, sums to 1. Therefore, the integral simplifies to integrating 2t from 0 to 1, which is straightforward.

So the exact answer is 1. The numerical approximation would then be 1.0000000000. But let me check with a numerical approximation to confirm. If I compute the integral numerically, does it equal 1?

Alternatively, maybe there's a mistake in the substitution. Let me test with a simple case. Suppose we take x from -a to a, and the integrand is f(x). If f(-x) + f(x) = 1, then the integral from -a to a would be a^2. Wait, in our case, after substitution, the integral becomes 1. But let's check with a=1. If f(x) + f(-x) =1, then ∫_{-a}^a f(x) dx = ∫_{-a}^a [f(x) + f(-x)] / 2 dx * 2? Wait, no. Wait, in our case, when we split the integral into two parts, each part's integrand adds up to 1. So the total is 1. So the integral is 1. So the exact answer is 1. Therefore, the numerical approximation is exactly 1.0000000000.

But to be thorough, maybe I should compute the integral numerically. Let's approximate the integral using a simple method. For example, take x=0. The integrand at x=0 is sin(0)/(sinh(0)+sin(0)) = 0/0. Hmm, indeterminate. Need to compute the limit as x approaches 0 from the right. Using L’Hospital’s Rule: For x approaching 0+, t = sqrt(x) approaches 0. The integrand becomes sin(t)/(sinh(t) + sin(t)). As t→0, sin(t) ≈ t - t^3/6, sinh(t) ≈ t + t^3/6. So sinh(t) + sin(t) ≈ 2t. So the integrand ≈ t/(2t) = 1/2. So near x=0, the integrand approaches 1/2. Similarly, for x approaching 0 from the left, the integrand is sinh(t)/(sin(t) + sinh(t)) ≈ t/(2t) = 1/2. So the function is continuous at x=0 with value 1/2.

Similarly, at x=1, the integrand is sin(1)/(sinh(1) + sin(1)) which is a finite value. So the integrand is well-behaved over the interval. But since the analytical result is 1, the numerical approximation should be very close to 1. Let me check with a simple approximation. For example, using the trapezoidal rule with a few intervals. But since the integral is exactly 1, any numerical method should confirm that. Therefore, the numerical answer is 1.0000000000.
</think>

{"answer": "1", "numerical_answer": "1.0000000000"}