Let's start by analyzing the integral:
\[
\int_1^2\frac{9x+4}{x^5+3x^2+x}\ dx
\]

First, factor the denominator:
\[
x^5 + 3x^2 + x = x(x^4 + 3x + 1)
\]
So, the integrand is:
\[
\frac{9x+4}{x(x^4 + 3x + 1)}
\]

Let's attempt partial fraction decomposition.  
Set:
\[
\frac{9x+4}{x(x^4 + 3x + 1)} = \frac{A}{x} + \frac{Bx^3 + Cx^2 + Dx + E}{x^4 + 3x + 1}
\]

Multiply both sides by the denominator:
\[
9x+4 = A(x^4 + 3x + 1) + (Bx^3 + Cx^2 + Dx + E)x
\]
\[
9x+4 = A x^4 + 3A x + A + B x^4 + C x^3 + D x^2 + E x
\]

\[
= (A + B) x^4 + C x^3 + D x^2 + (3A + E) x + A
\]

Set this equal to the left side, and compare coefficients:
\[
9x + 4 = (A+B)x^4 + Cx^3 + Dx^2 + (3A+E)x + A
\]

Match powers of \(x\):

- \(x^4\): \(A+B=0 \implies B = -A\)
- \(x^3\): \(C = 0\)
- \(x^2\): \(D = 0\)
- \(x^1\): \(3A + E = 9\)
- Constant: \(A = 4\)

So \(A = 4\), \(B = -4\), \(C = 0\), \(D = 0\), \(3A + E = 9 \implies 12 + E = 9 \implies E = -3\).

So:

\[
\frac{9x+4}{x(x^4 + 3x + 1)} = \frac{4}{x} + \frac{(-4)x^3 + (-3)}{x^4 + 3x + 1}
\]

Or:

\[
\frac{9x+4}{x(x^4 + 3x + 1)} = \frac{4}{x} + \frac{ -4x^3 - 3 }{ x^4 + 3x + 1 }
\]

So:

\[
\int_1^2\frac{9x+4}{x^5+3x^2+x}\ dx = \int_1^2 \frac{4}{x} \ dx + \int_1^2 \frac{-4x^3 - 3}{x^4 + 3x + 1}\ dx
\]

Let's compute both terms:

The first term:
\[
\int_1^2 \frac{4}{x} dx = 4 \ln x \Big|_1^2 = 4 \ln 2
\]

The second term:
\[
\int_1^2 \frac{-4x^3 - 3}{x^4 + 3x + 1} dx
\]

Let’s split the numerator:
\[
\frac{-4x^3 - 3}{x^4 + 3x + 1} = \frac{-4x^3}{x^4 + 3x + 1} - \frac{3}{x^4 + 3x + 1}
\]

For the first part,

Let’s substitute \(u = x^4 + 3x + 1\), then
\[
\frac{du}{dx} = 4x^3 + 3
\]
So
\[
-4x^3dx = -du + 3dx
\]

So

\[
-4x^3dx = -du + 3dx
\implies \frac{-4x^3}{x^4 + 3x + 1} dx = \frac{ - du + 3 dx }{x^4 + 3x + 1}
= - \frac{du}{u} + \frac{3 dx}{u}
\]

Wait, that's equivalent to:

\[
\frac{-4x^3 - 3}{x^4 + 3x + 1} dx = \frac{ -4x^3 }{ x^4 + 3x + 1 } dx - \frac{3}{x^4 + 3x + 1} dx 
\]

From above \(du = 4x^3 dx + 3 dx\)
So \(4x^3 dx = du - 3 dx\), so \(-4x^3 dx = -du + 3 dx\).

So:

\[
\frac{-4x^3 - 3}{x^4 + 3x + 1}dx = - \frac{du}{u}
\]

Therefore,

\[
\int_1^2 \frac{-4x^3 - 3}{x^4 + 3x + 1}dx = - \int_{x=1}^{x=2} \frac{1}{u} du
= - [\ln (x^4 + 3x + 1)]_1^2
= - (\ln (2^4 + 3\times2 + 1) - \ln (1^4 + 3\times1 + 1))
= - (\ln (16+6+1) - \ln(1+3+1))
= - (\ln 23 - \ln 5)
= - \ln(23/5)
\]

Putting it all together:

\[
\int_1^2\frac{9x+4}{x^5+3x^2+x}dx = 4\ln 2 - \ln \left(\frac{23}{5}\right)
= 4\ln 2 + \ln\left(\frac{5}{23}\right)
= \ln\left(16 \cdot \frac{5}{23}\right) = \ln\left( \frac{80}{23} \right )
\]

So the exact answer is:
\[
\boxed{\,\ln\left(\dfrac{80}{23}\right) \,}
\]

Now, the numerical value:

\[
\ln\left(\frac{80}{23}\right) = \ln(80) - \ln(23)
\]

Calculate:

- \(\ln(80) = 4.38202663467\)
- \(\ln(23) = 3.13549421593\)

So,

\[
4.38202663467 - 3.13549421593 = 1.24653241874
\]

Rounded to 10 decimal places: 1.2465324187

Final answer in JSON format:
```
{"answer": "\\ln\\left(\\dfrac{80}{23}\\right)", "numerical_answer": "1.2465324187"}
```