Let's evaluate the definite integral:
\[
I = \int_0^1 \arcsin(0.5x)\arccos x\, dx
\]

**Step 1: Analytic calculation**

Let’s use integration by parts.

Let:
- \( u = \arcsin(0.5x) \implies du = \frac{0.5}{\sqrt{1 - (0.5x)^2}} dx = \frac{0.5}{\sqrt{1 - 0.25x^2}} dx \)
- \( dv = \arccos x\, dx \implies v = x\arccos x - \int x \cdot \left(-\frac{1}{\sqrt{1-x^2}}\right) dx = x\arccos x + \int \frac{x\, dx}{\sqrt{1-x^2}} \)

But this is a bit complex. Instead, swap:
Let
- \( u = \arccos x \implies du = -\frac{1}{\sqrt{1-x^2}} dx \)
- \( dv = \arcsin(0.5x)\, dx \), so \( v = \int \arcsin(0.5x) dx \)

Let’s compute \( v \):

Let’s compute \( \int \arcsin(ax) dx \):

Let \( I_1=\int \arcsin(ax) dx \).
Use integration by parts:
- \( f = \arcsin(ax) \implies df = \frac{a}{\sqrt{1-(ax)^2}} dx \)
- \( dg = dx \implies g = x \)

So
\[
I_1 = x\arcsin(ax) - \int x \cdot \frac{a}{\sqrt{1-(ax)^2}} dx
\]
Let \( t = ax \to x = t/a, dx = dt/a \):

So
\[
\int x \frac{a}{\sqrt{1-(ax)^2}} dx
= \int x \frac{a}{\sqrt{1 - (ax)^2}} dx
= \int \frac{x a}{\sqrt{1-(ax)^2}} dx
= \int \frac{t}{\sqrt{1-t^2}} \frac{dt}{a}
= \int \frac{t}{a \sqrt{1-t^2}} dt
\]

But:
\[
\int \frac{t}{\sqrt{1-t^2}} dt
\]
Let \( u = 1-t^2 \implies du = -2t dt \implies -\frac12 du = t dt \)
Thus,
\[
\int \frac{t}{\sqrt{1-t^2}} dt = -\frac12 \int u^{-1/2} du = -\frac12 \cdot 2 u^{1/2} = -\sqrt{1-t^2}
\]

Therefore,
\[
\int x \frac{a}{\sqrt{1-(ax)^2}} dx = \frac{-1}{a} \sqrt{1 - (ax)^2}
\]

So,
\[
\int \arcsin(ax) dx = x \arcsin(ax) + \frac{1}{a}\sqrt{1 - (ax)^2} + C
\]

Set \( a = 0.5 \), then:

\[
v = x\arcsin(0.5x) + 2\sqrt{1 - 0.25x^2}
\]

Apply integration by parts:

\[
I = \int_0^1 \arcsin(0.5x)\arccos x\, dx = \left[u v\right]_0^1 - \int_0^1 v\, du
\]
where 
- \( u = \arccos x \)
- \( v = x\arcsin(0.5x) + 2\sqrt{1 - 0.25x^2} \)
- \( du = -\frac{1}{\sqrt{1-x^2}} dx \)

**Compute the boundary term:**

\[
\left[u v\right]_0^1 = \left[ \arccos x \left(x\arcsin(0.5x) + 2\sqrt{1 - 0.25x^2}\right)\right]_0^1
\]

At \( x = 1 \):
- \( \arccos 1 = 0 \)
- \( \arcsin(0.5 \times 1) = \arcsin(0.5) = \frac{\pi}{6} \)
- \( \sqrt{1 - 0.25 \times 1^2} = \sqrt{1 - 0.25} = \sqrt{0.75} = \frac{\sqrt{3}}{2} \)

So the term at \( x=1 \) is \( 0 \).

At \( x = 0 \):
- \( \arccos 0 = \frac{\pi}{2} \)
- \( \arcsin(0) = 0 \)
- \( \sqrt{1 - 0} = 1 \)

So the term at \( x=0 \) is \( \frac{\pi}{2} \times (0 + 2 \times 1) = \pi \)

Therefore,
\[
\left[u v\right]_0^1 = 0 - \pi = -\pi
\]

**Now compute the integral:**
\[
-\int_0^1 v\, du = -\int_0^1 \left[ x\arcsin(0.5x) + 2\sqrt{1-0.25x^2} \right] \left(-\frac{1}{\sqrt{1-x^2}}\right) dx
\]
\[
= \int_0^1 \left[ x\arcsin(0.5x) + 2\sqrt{1-0.25x^2} \right] \frac{1}{\sqrt{1-x^2}} dx
\]
\[
= \int_0^1 \frac{x\arcsin(0.5x)}{\sqrt{1-x^2}} dx + 2 \int_0^1 \frac{\sqrt{1-0.25x^2}}{\sqrt{1-x^2}} dx
\]

Let’s call

\[
I_1 = \int_0^1 \frac{x\arcsin(0.5x)}{\sqrt{1-x^2}} dx
\]
\[
I_2 = \int_0^1 \frac{\sqrt{1-0.25x^2}}{\sqrt{1-x^2}} dx
\]

So,
\[
I = -\pi + I_1 + 2 I_2
\]

---

Let's calculate \( I_2 \) first.

Let \( x = \sin \theta \), so as \( x \) goes from 0 to 1, \( \theta \) goes from 0 to \( \frac{\pi}{2} \):

- \( dx = \cos \theta d\theta \)
- \( \sqrt{1-x^2} = \cos\theta \)
- \( 1 - 0.25x^2 = 1 - 0.25\sin^2\theta \)

So,
\[
I_2 = \int_{x=0}^{x=1} \frac{\sqrt{1-0.25x^2}}{\sqrt{1-x^2}} dx = \int_{\theta=0}^{\theta=\pi/2} \frac{\sqrt{1-0.25\sin^2\theta}}{\cos\theta} \cos\theta d\theta = \int_0^{\pi/2} \sqrt{1-0.25\sin^2\theta} d\theta
\]

This is (up to a scaling) the complete elliptic integral of the second kind:

\[
\int_0^{\pi/2} \sqrt{1 - k^2 \sin^2 \theta} d\theta = E(k)
\]
with \( k^2 = 0.25 \implies k = 0.5 \).

So,
\[
I_2 = E(0.5)
\]
where \( E(m) \) is the complete elliptic integral of the second kind.

---

Now, \( I_1 \):

Again, split up the numerator \( x\arcsin(0.5x) \), set \( x = \sin\theta \):

- As above, \( dx = \cos\theta d\theta \)
- \( \sqrt{1-x^2} = \cos\theta \)
So,
\[
I_1 = \int_0^1 \frac{x\arcsin(0.5x)}{\sqrt{1-x^2}}dx = \int_{\theta=0}^{\theta=\frac{\pi}{2}} \frac{\sin\theta \arcsin(0.5\sin\theta)}{\cos\theta} \cos\theta d\theta = \int_{0}^{\pi/2} \sin\theta \arcsin(0.5\sin\theta) d\theta
\]
Let’s denote this:

\[
I_1 = \int_0^{\frac{\pi}{2}} \sin\theta\, \arcsin(0.5\sin\theta) d\theta
\]

Let’s try substitution to compute this integral.

Let’s let \( \phi = \arcsin(0.5 \sin\theta) \), then \( \sin\phi = 0.5\sin\theta \).

But expressing everything in terms of \( \phi \) gets involved. An alternative is to refer to known results for these integrals, or else leave this as it is.

Alternatively, integrate by parts:
Let
- \( f = \arcsin(0.5\sin\theta) \implies df = \frac{0.5\cos\theta}{\sqrt{1 - (0.5\sin\theta)^2}} d\theta = \frac{0.5\cos\theta}{\sqrt{1 - 0.25 \sin^2\theta}} d\theta \)
- \( dg = \sin\theta d\theta \implies g = -\cos\theta \)

So,

\[
I_1 = \int_0^{\pi/2} \sin\theta\, \arcsin(0.5\sin\theta) d\theta \\
= \left. -\cos\theta\, \arcsin(0.5\sin\theta)\right|_0^{\pi/2} + \int_0^{\pi/2} \cos\theta \cdot \frac{0.5\cos\theta}{\sqrt{1 - 0.25\sin^2\theta}} d\theta
\]
\[
= -\cos\theta\, \arcsin(0.5\sin\theta) \Big|_0^{\pi/2} + 0.5\int_0^{\pi/2} \frac{\cos^2\theta}{\sqrt{1 - 0.25\sin^2\theta}} d\theta
\]

Let's evaluate the first term:
- At \( \theta = 0 \): \( \cos 0 = 1 \), \( \sin 0 = 0 \), \( \arcsin(0) = 0 \), so \( -1\times 0 = 0 \)
- At \( \theta = \frac{\pi}{2} \): \( \cos(\frac{\pi}{2}) = 0 \), \( \sin(\frac{\pi}{2}) = 1 \), \( \arcsin(0.5) = \frac{\pi}{6} \), so \( 0\times \cdots = 0 \)

So, this boundary term is 0.

Thus,
\[
I_1 = 0.5\int_0^{\pi/2} \frac{\cos^2\theta}{\sqrt{1-0.25\sin^2\theta}} d\theta
\]

Now, recall that \( \cos^2\theta = 1 - \sin^2\theta \), so:

\[
I_1 = 0.5\int_0^{\pi/2}\frac{d\theta}{\sqrt{1-0.25\sin^2\theta}} - 0.5\int_0^{\pi/2}\frac{\sin^2\theta\, d\theta}{\sqrt{1-0.25\sin^2\theta}}
\]

Let’s call:
- \( J_1 = \int_0^{\pi/2}\frac{d\theta}{\sqrt{1-0.25\sin^2\theta}} \)
- \( J_2 = \int_0^{\pi/2}\frac{\sin^2\theta\, d\theta}{\sqrt{1-0.25\sin^2\theta}} \)

Therefore,
\[
I_1 = 0.5 (J_1 - J_2)
\]

But \( J_1 \) is the complete elliptic integral of the first kind:

\[
J_1 = K(0.5)
\]

Now \( J_2 \). Let’s express this in terms of complete elliptic integrals:

Recall that:
\[
\int_0^{\pi/2} \frac{\sin^2 \theta}{\sqrt{1 - k^2 \sin^2\theta}} d\theta = \frac{1}{k^2} [ E(k) - (1 - k^2) K(k) ]
\]
(See tables of elliptic integrals.)

So, with \( k = 0.5 \), \( k^2 = 0.25 \):

\[
J_2 = \int_0^{\pi/2} \frac{\sin^2\theta}{\sqrt{1 - 0.25 \sin^2 \theta}} d\theta = \frac{1}{0.25} \left[ E(0.5) - (1 - 0.25) K(0.5) \right]
= 4 [ E(0.5) - 0.75 K(0.5) ]
\]

Therefore,
\[
I_1 = 0.5 [ K(0.5) - 4 ( E(0.5) - 0.75 K(0.5) ) ] = 0.5 [ K(0.5) - 4 E(0.5) + 3 K(0.5) ) ] = 0.5 [ 4 K(0.5) - 4 E(0.5) ] = 2 [ K(0.5) - E(0.5) ]
\]

So

\[
I_1 = 2 ( K(0.5) - E(0.5) )
\]
and
\[
I_2 = E(0.5)
\]

Recall from above:
\[
I = -\pi + I_1 + 2I_2 = -\pi + 2 ( K(0.5) - E(0.5) ) + 2 E(0.5 ) = -\pi + 2K(0.5)
\]

Thus, the final answer is:
\[
I = 2 K(0.5) - \pi
\]

---

**Step 2: Numerical approximation**

The complete elliptic integral of the first kind \( K(0.5) \) is approximately:
\[
K(0.5) \approx 1.6857503548
\]

Thus,
\[
I \approx 2 \times 1.6857503548 - \pi \approx 3.3715007096 - 3.1415926536 = 0.2299080560
\]

---

**Step 3: JSON Output**

```json
{"answer": "2 K \\left( \\frac{1}{2} \\right) - \\pi", "numerical_answer": "0.2299080560"}
```