Let’s solve the integral:
\[
I = \int_{0}^{2} x^{-1/4} (2-x)^{-3/4} \sin\left(\sqrt[4]{x(2-x)}\right)\,dx
\]

**Step 1: Substitution**

Let us use the substitution:
\[
x = 2 \sin^2 \theta, \quad \theta \in [0, \pi/2]
\]
Then,
\[
dx = 4\sin\theta\cos\theta\, d\theta = 2\sin(2\theta) d\theta
\]
Compute \(x(2-x)\):
\[
x(2-x) = 2\sin^2\theta (2 - 2\sin^2\theta) = 4\sin^2\theta\cos^2\theta = (\sin 2\theta)^2
\]
So,
\[
\sqrt[4]{x(2-x)} = \sqrt{|\sin 2\theta|}
\]
But \(\sin 2\theta \ge 0\) for \(\theta\in [0,\pi/2]\), so:
\[
\sqrt[4]{x(2-x)} = (\sin 2\theta)^{1/2}
\]

Now, rewrite the powers:

- \(x^{-1/4} = (2\sin^2\theta)^{-1/4} = 2^{-1/4} \sin^{-1/2}\theta\)
- \((2-x)^{-3/4} = (2\cos^2\theta)^{-3/4} = 2^{-3/4} \cos^{-3/2}\theta\)

So the integral becomes:
\[
I = \int_{x=0}^{x=2} x^{-1/4}(2-x)^{-3/4} \sin\left((x(2-x))^{1/4}\right) dx
\]
\[
= \int_{\theta=0}^{\theta=\pi/2} 2^{-1/4} \sin^{-1/2}\theta \cdot 2^{-3/4} \cos^{-3/2}\theta \cdot \sin\left((\sin 2\theta)^{1/2}\right) \cdot 2\sin 2\theta d\theta
\]
\[
= 2^{-1/4-3/4+1} \int_{0}^{\pi/2} \sin^{-1/2}\theta \cos^{-3/2}\theta \cdot \sin\left((\sin 2\theta)^{1/2}\right) \cdot \sin 2\theta d\theta
\]
\[
= 2^{0} \int_{0}^{\pi/2} \sin^{-1/2}\theta \cos^{-3/2}\theta \cdot \sin\left((\sin 2\theta)^{1/2}\right) \cdot \sin 2\theta d\theta 
\]

But:
\[
\sin 2\theta = 2\sin\theta \cos\theta
\]
So:
\[
\sin^{-1/2}\theta \cos^{-3/2}\theta \cdot \sin 2\theta = \sin^{-1/2}\theta \cos^{-3/2}\theta \cdot 2\sin\theta \cos\theta = 2 \sin^{1/2}\theta \cos^{-1/2}\theta
\]
Hence:
\[
I = 2 \int_{0}^{\pi/2} \sin^{1/2}\theta \cos^{-1/2}\theta \sin\left((\sin 2\theta)^{1/2}\right) d\theta
\]

Let’s now perform the substitution \(u = \sin 2\theta\), with \(\theta\) from 0 to \(\pi/2\), \(u\) runs from 0 to 1.
\[
du = 2\cos 2\theta d\theta
\]
But we might try another substitution to get a Beta-integral-like form.

Alternatively, let’s let \(x = 2t\), \(dx = 2 dt\), \(t \in [0, 1]\):
\[
I = \int_{x=0}^{x=2} x^{-1/4}(2-x)^{-3/4}\sin\left((x(2-x))^{1/4}\right)dx \\
= 2\int_{t=0}^{1} (2t)^{-1/4}[2(1-t)]^{-3/4} \sin\left([(2t)(2(1-t))]^{1/4}\right) dt \\
= 2 \cdot 2^{-1/4} \cdot 2^{-3/4} \int_{0}^{1} t^{-1/4} (1-t)^{-3/4} \sin\left([4t(1-t)]^{1/4}\right) dt \\
= 2 \cdot 2^{-1} \int_{0}^{1} t^{-1/4} (1-t)^{-3/4} \sin\left(2^{1/2}(t(1-t))^{1/4}\right) dt \\
= \int_{0}^{1} t^{-1/4} (1-t)^{-3/4} \sin\left(2^{1/2}(t(1-t))^{1/4}\right) dt
\]

But this is not quite what’s in the integral. Actually, notice that the argument of sine is:
\[
\sqrt[4]{x(2-x)} = [x(2-x)]^{1/4}
\]
Let’s check this: with \(x=2t\), \(x(2-x)=2t(2-2t)=4t(1-t)\):

So,
\[
I = \int_0^1 t^{-1/4}(1-t)^{-3/4}\sin \Big( [4t(1-t)]^{1/4} \Big) dt
\]

So the integral becomes:
\[
I = \int_0^1 t^{-1/4}(1-t)^{-3/4} \sin \left( 2^{1/2} (t(1-t))^{1/4} \right) dt
\]

Recognize a standard integral representation of the Beta function with a sine modulation.

**Step 2: Expansion**

Expand the sine term in Taylor series:
\[
\sin\left(a z^{1/4}\right) = \sum_{k=0}^\infty \frac{(-1)^k}{(2k+1)!} a^{2k+1} z^{(2k+1)/4}
\]
with \(z = 4t(1-t)\), \(a = 1\):

So,
\[
I = \int_0^1 t^{-1/4}(1-t)^{-3/4} \sum_{k=0}^\infty \frac{(-1)^k}{(2k+1)!} \left(4t(1-t)\right)^{(2k+1)/4} dt
\]

\[
= \sum_{k=0}^\infty \frac{(-1)^k 4^{(2k+1)/4}}{(2k+1)!} \int_0^1 t^{-1/4} t^{(2k+1)/4} (1-t)^{-3/4} (1-t)^{(2k+1)/4} dt
\]
\[
= \sum_{k=0}^\infty \frac{(-1)^k 4^{(2k+1)/4}}{(2k+1)!} \int_0^1 t^{k/2} (1-t)^{k/2 - 1/2} dt
\]

But \(4^{(2k+1)/4} = 2^{(2k+1)/2} = 2^{k + 1/2}\).

So,
\[
I = \sum_{k=0}^\infty \frac{(-1)^k 2^{k+1/2}}{(2k+1)!} \int_0^1 t^{k/2}(1-t)^{k/2 - 1/2} dt
\]

But
\[
\int_0^1 t^{\alpha-1} (1-t)^{\beta-1} dt = B(\alpha, \beta) = \frac{\Gamma(\alpha)\Gamma(\beta)}{\Gamma(\alpha+\beta)}
\]

We have
\[
t^{k/2} = t^{k/2}, \quad (1-t)^{k/2 - 1/2}
\]
Corresponds to \(\alpha = 1 + \frac{k}{2}\), \(\beta = \frac{1}{2} + \frac{k}{2}\):

So,
\[
I = \sum_{k=0}^\infty \frac{(-1)^k 2^{k+1/2}}{(2k+1)!} \cdot B\left(1 + \frac{k}{2}, \frac{1}{2} + \frac{k}{2}\right)
\]
\[
= \sum_{k=0}^\infty \frac{(-1)^k 2^{k+1/2}}{(2k+1)!} \cdot \frac{\Gamma(1 + k/2) \Gamma(1/2 + k/2)}{\Gamma(3/2 + k)}
\]

**Step 3: Final analytic answer**

So, the exact answer is:
\[
\boxed{
I = \sum_{k=0}^\infty \frac{(-1)^k \, 2^{k+1/2} \, \Gamma(1 + k/2) \Gamma(1/2 + k/2)}{(2k+1)! \, \Gamma(3/2 + k)}
}
\]

**Step 4: Numerical approximation**

Let’s compute the sum numerically. We only need the first few terms for good accuracy:

- For \(k=0\):

\[
(-1)^0 \cdot 2^{0+1/2} / 1! = \sqrt{2} / 1 = 1.414213562
\]
\[
\Gamma(1) = 1, \quad \Gamma(1/2) = \sqrt{\pi} \approx 1.772453851,
\quad \Gamma(3/2) = 0.5\sqrt{\pi} \approx 0.886226925
\]
First term:
\[
T_0 = \frac{\sqrt{2} \cdot 1 \cdot \sqrt{\pi}}{1 \cdot 0.886226925} \approx \frac{1.414213562 \cdot 1.772453851}{0.886226925}
\]
Calculate numerator: \(1.414213562 \times 1.772453851 = 2.507299080\)
Divide: \(2.507299080 / 0.886226925 = 2.830025126\)

- For \(k=1\):

\[
(-1)^1 2^{1+1/2} = -2^{1.5} = -2.82842712, (2k+1)! = 3! = 6
\]
\[
\Gamma(1+0.5) = \Gamma(1.5) = 0.886226925, \quad \Gamma(1/2+0.5) = \Gamma(1) = 1, \quad \Gamma(2.5) = (1.5)\Gamma(1.5) = 1.329340388
\]
So,
\[
T_1 = \frac{-2.828427124 \cdot 0.886226925 \cdot 1}{6 \cdot 1.329340388}
\]
Compute numerator: \(2.828427124 \cdot 0.886226925 = 2.507299080\), but negative, so -2.507299080
\[
T_1 = -2.507299080 / (6 \times 1.329340388) = -2.507299080 / 7.976042328 = -0.314428923
\]

- For \(k=2\):

\(
(-1)^2 2^{2+1/2} = 2^{2.5} = 5.656854249, (2k+1)! = 5! = 120
\)
\(\Gamma(2) = 1, \Gamma(1.5) = 0.886226925, \Gamma(3.5) = (2.5)\Gamma(2.5) = 2.5 \times 1.329340388 = 3.323350969\)

\[
T_2 = \frac{5.656854249 \cdot 1 \cdot 0.886226925}{120 \cdot 3.323350969}
\]
\[
Num: 5.656854249 \cdot 0.886226925 = 5.014598159
\]
\[
Denom: 120 \cdot 3.323350969 = 398.8021163
\]
\[
T_2 = 5.014598159 / 398.8021163 = 0.012574931
\]

- For \(k=3\):

\[
(-1)^3 2^{3+1/2} = -2^{3.5} = -11.31370850, (2k+1)! = 7! = 5040
\]
\(\Gamma(2.5) = 1.329340388, \Gamma(2) = 1, \Gamma(4.5) = (3.5)\Gamma(3.5) = 3.5 \times 3.323350969 = 11.63172839\)
\[
T_3 = \frac{-11.31370850 \cdot 1.329340388 \cdot 1}{5040 \cdot 11.63172839} 
\]
Numerator: \(11.31370850 \cdot 1.329340388 = 15.02379448\), so -15.02379448
Denominator: \(5040 \cdot 11.63172839 = 58606.91614\)
\[
T_3 = -15.02379448 / 58606.91614 = -0.000256493
\]

- For \(k=4\):

\[
(-1)^4 2^{4+1/2} = 2^{4.5} = 22.627416997, (2k+1)! = 9! = 362880
\]
\(\Gamma(3) = 2, \Gamma(2.5) = 1.329340388, \Gamma(5.5) = (4.5)\Gamma(4.5) = 4.5 \cdot 11.63172839 = 52.34277777\)
\[
T_4 = \frac{22.627416997 \cdot 2 \cdot 1.329340388}{362880 \cdot 52.34277777}
\]
Numerator: \(22.627416997 \cdot 2 = 45.254833994\), then times 1.329340388 = 60.09322543
Denominator: \(362880 \cdot 52.34277777 = 19,011,383.65\)
\[
T_4 = 60.09322543 / 19,011,383.65 = 0.000003163
\]

Summing the first five terms:
\[
S \approx 2.830025126 - 0.314428923 + 0.012574931 - 0.000256493 + 0.000003163 
= 2.528947804
\]

Adding more terms yields rapidly smaller corrections.

**Thus, up to 10 decimal places:**
\[
I \approx 2.5289478040
\]

**Step 5: JSON output**

```json
{"answer": "\\sum_{k=0}^\\infty \\frac{(-1)^k \\, 2^{k+1/2} \\, \\Gamma\\left(1+\\frac{k}{2}\\right) \\Gamma\\left(\\frac{1}{2}+\\frac{k}{2}\\right)}{(2k+1)! \\, \\Gamma\\left(\\frac{3}{2}+k\\right)}", "numerical_answer": "2.5289478040"}
```