<think>
Okay, so I need to compute the definite integral from 0 to π/2 of ln(sin x) divided by cos squared x dx. Hmm, let me think about how to approach this. The integral is ∫₀^{π/2} [ln(sin x)] / cos²x dx. 

First, I remember that integrating functions involving logarithms and trigonometric functions can sometimes be tricky. Maybe integration by parts would work here? Let me recall the formula: ∫u dv = uv - ∫v du. Let's choose u and dv. 

Let me set u = ln(sin x). Then du would be (cos x / sin x) dx, right? Because the derivative of ln(sin x) is (1/sin x)*cos x. Then dv would be 1/cos²x dx. The integral of dv is v, so integrating 1/cos²x dx is tan x, since the integral of sec²x is tan x. 

So applying integration by parts: uv - ∫v du. That would be ln(sin x)*tan x evaluated from 0 to π/2 minus the integral of tan x * (cos x / sin x) dx. Let's simplify that. 

First, the boundary term: [ln(sin x) * tan x] from 0 to π/2. Let's check the limits. As x approaches π/2, sin x approaches 1, so ln(1) is 0, and tan x approaches infinity. But 0 times infinity is an indeterminate form. Hmm, need to check the limit. Similarly, as x approaches 0, sin x approaches 0, so ln(sin x) approaches -infinity, and tan x approaches 0. So again, 0 times -infinity. So maybe the boundary term is problematic? Let me see. Let's compute the limit as x approaches π/2 from the left. Let x = π/2 - ε, where ε approaches 0+. Then sin x = sin(π/2 - ε) = cos ε ≈ 1 - ε²/2. So ln(sin x) ≈ ln(1 - ε²/2) ≈ -ε²/2. Tan x = tan(π/2 - ε) = cot ε ≈ 1/ε. So the product is approximately (-ε²/2)*(1/ε) = -ε/2, which approaches 0 as ε approaches 0. So the upper limit term is 0. 

Now the lower limit as x approaches 0+. Let x approach 0 from the right. Then sin x ≈ x, so ln(sin x) ≈ ln x. Tan x ≈ x. So the product is x ln x, which as x approaches 0+ is 0 * (-infty). The limit of x ln x as x→0+ is 0, since ln x approaches -infty but x approaches 0, and x dominates. So the boundary term is 0 - 0 = 0. So the boundary terms vanish. 

So now the integral becomes -∫ tan x * (cos x / sin x) dx. Let's simplify the integrand. tan x is sin x / cos x, so multiplying by cos x / sin x gives (sin x / cos x) * (cos x / sin x) = 1. So the integral becomes -∫ 1 dx from 0 to π/2. Wait, that's too simple? So the integral is - [x] from 0 to π/2, which is - (π/2 - 0) = -π/2. 

Wait, but that seems too straightforward. Let me check again. The integral after integration by parts is -∫ v du. v is tan x, du is (cos x / sin x) dx. So v du is tan x * (cos x / sin x) dx. Let's compute tan x * (cos x / sin x). tan x is sin x / cos x, so substituting in, we get (sin x / cos x) * (cos x / sin x) dx. The sin x cancels with sin x, cos x cancels with cos x, so it's 1 dx. Therefore, the integral is -∫1 dx from 0 to π/2, which is - (π/2 - 0) = -π/2. 

But wait, the original integral was ∫ [ln(sin x)] / cos²x dx from 0 to π/2. So according to this, the integral is -π/2. But let me verify this with a numerical approximation. Let's compute the integral numerically. Let's take x = π/4, for example. The integrand is ln(sin(π/4)) / cos²(π/4) = ln(√2/2) / ( (√2/2)^2 ) = ln(1/√2) / (1/2) = (- (1/2) ln 2 ) / (1/2) = -ln 2. So at x=π/4, the integrand is -ln 2 ≈ -0.6931. The integral over 0 to π/2 would be the area under this curve. But according to the analytical result, it's -π/2 ≈ -1.5708. Let me check with another approach.

Alternatively, maybe there's a mistake in the integration by parts. Let me redo the steps. Let u = ln(sin x), dv = dx / cos²x. Then du = (cos x / sin x) dx, v = tan x. Then integration by parts gives uv| from 0 to π/2 - ∫ v du. The uv term is [ln(sin x) * tan x] from 0 to π/2. As we saw, both limits go to 0. Then the remaining integral is -∫ tan x * (cos x / sin x) dx. Simplify tan x: tan x = sin x / cos x. So multiplying by cos x / sin x gives (sin x / cos x) * (cos x / sin x) = 1. So the integral becomes -∫1 dx from 0 to π/2, which is -π/2. So the result is -π/2. 

But wait, when I think about the integrand, ln(sin x) is negative over (0, π/2) because sin x is between 0 and 1, so ln(sin x) is negative. Then divided by cos²x, which is positive. So the integrand is negative over the entire interval. Therefore, the integral should be negative, which matches the result -π/2. But let me check with a numerical approximation. Let's approximate the integral numerically. Let's use substitution. Let me compute the integral numerically. Let's split the integral into parts. For example, approximate ∫₀^{π/2} ln(sin x)/cos²x dx. Let's use substitution t = x, but maybe another substitution. Alternatively, use series expansion? Hmm, maybe not. Alternatively, use numerical integration techniques like Simpson's rule. Let's approximate the integral numerically. Let's take a few points. Let's take x = π/4, as before, the integrand is -ln 2 ≈ -0.6931. At x = π/6, sin x = 1/2, so ln(1/2) = -ln 2, cos²x = (√3/2)^2 = 3/4, so integrand is (-ln 2)/(3/4) = - (4/3) ln 2 ≈ -1.8484. At x approaching π/2, the integrand approaches 0 (since ln(sin x) approaches 0, and cos²x approaches 0, but the limit is 0). At x approaching 0, ln(sin x) approaches -infty, but divided by cos²x which approaches 1, so the integrand approaches -infty. Wait, but near x=0, the integrand is ln(sin x)/cos²x ≈ ln x / 1, which tends to -infty. But the integral from 0 to π/2 of ln x dx would be divergent, but in our case, the integrand is ln(sin x)/cos²x. Wait, but sin x ~ x as x approaches 0, so ln(sin x) ~ ln x, and cos²x ~ 1 - x², so near 0, the integrand behaves like ln x / (1 - x²) ≈ ln x (1 + x² + ...). So the integrand near 0 is approximately ln x, which integrates to x ln x - x. The integral of ln x from 0 to a is a ln a - a - (lim_{x→0} x ln x - x) = a ln a - a - (0 - 0) = a ln a - a. As a approaches 0, this approaches 0 -0 = 0. Wait, but the integral of ln x from 0 to a is (x ln x - x) evaluated at a and 0. The limit as x approaches 0 of x ln x is 0, so the integral from 0 to a is a ln a - a. So if the integrand near 0 is ln x, then the integral would converge? Wait, but ln x is integrable over (0, a) because the integral of ln x dx is x ln x - x, which is finite as x approaches 0. So even though ln x approaches -infty, the integral is finite. So the integral ∫₀^{π/2} ln(sin x)/cos²x dx is convergent. 

But according to our analytical result, it's -π/2 ≈ -1.5708. Let me check with a numerical approximation. Let's compute the integral numerically. Let's use substitution t = tan x. Let x = arctan t, so dx = dt/(1 + t²). When x=0, t=0; x=π/2, t approaches infinity. Then sin x = t / sqrt(1 + t²), cos x = 1 / sqrt(1 + t²). So the integrand becomes ln(t / sqrt(1 + t²)) / (1 / (1 + t²)) ) * (dt / (1 + t²)). Wait, let's compute each part. The integrand is [ln(sin x)] / cos²x dx. Substituting sin x = t / sqrt(1 + t²), cos²x = 1 / (1 + t²). So [ln(t / sqrt(1 + t²))] / (1 / (1 + t²)) * [dt / (1 + t²)]. Simplify this: [ln(t) - (1/2) ln(1 + t²)] * (1 + t²) * [dt / (1 + t²)] = [ln(t) - (1/2) ln(1 + t²)] dt. So the integral becomes ∫₀^∞ [ln t - (1/2) ln(1 + t²)] dt. Hmm, but this integral from 0 to infinity might be easier to handle. Let's split it into two integrals: ∫₀^∞ ln t dt - (1/2) ∫₀^∞ ln(1 + t²) dt. However, both of these integrals individually diverge. For example, ∫₀^∞ ln t dt is divergent (behaves like t ln t - t, which as t approaches infinity, goes to infinity). Similarly, ∫ ln(1 + t²) dt behaves like t ln t² for large t, which also diverges. So this substitution seems to lead to a divergent integral, which contradicts our previous conclusion that the original integral converges. Therefore, this substitution might not be helpful. Maybe another substitution is better. 

Alternatively, let's use substitution u = π/2 - x. Let x = π/2 - u. Then when x=0, u=π/2; x=π/2, u=0. The integral becomes ∫_{π/2}^0 [ln(sin(π/2 - u))]/cos²(π/2 - u) (-du) = ∫₀^{π/2} [ln(cos u)] / sin²u du. So the integral is equal to ∫₀^{π/2} ln(cos u)/sin²u du. Not sure if that helps. 

Alternatively, maybe use the Fourier series of ln(sin x). I recall that ln(sin x) can be expressed as -ln 2 - Σ_{n=1}^∞ (cos 2n x)/n. But integrating term by term might be complicated. Let's see. If we have ln(sin x) = -ln 2 - Σ_{n=1}^∞ (cos 2n x)/n, then the integrand becomes [-ln 2 - Σ (cos 2n x)/n] / cos²x. So the integral is -ln 2 ∫₀^{π/2} 1²x dx - Σ_{n=1}^∞ (1/n) ∫₀^{π/2} cos 2n x / cos²x dx. But integrating term by term might not be straightforward. Let's check the first integral: ∫ 1/cos²x dx = tan x, so from 0 to π/2, it diverges. Wait, but the original integral is ∫ ln(sin x)/cos²x dx, which we found analytically to be -π/2. But according to this series approach, the first term would be -ln 2 * ∫ sec²x dx, which diverges. So this suggests that maybe the series approach isn't suitable here. 

Alternatively, perhaps there's a mistake in the integration by parts. Let me check again. The integration by parts step: u = ln(sin x), dv = 1/cos²x dx. Then du = (cos x / sin x) dx, v = tan x. Then uv evaluated from 0 to π/2 is [ln(sin x) tan x] from 0 to π/2. As x approaches π/2, tan x approaches infinity, but ln(sin x) approaches ln 1 = 0. So the product is 0 * infty, which we evaluated earlier to be 0. Similarly, as x approaches 0, ln(sin x) approaches -infty, tan x approaches 0, so the product is 0. So the boundary terms are 0. Then the remaining integral is -∫ tan x * (cos x / sin x) dx. Simplify tan x as sin x / cos x, so multiplying by cos x / sin x gives 1. Therefore, the integral is -∫1 dx from 0 to π/2, which is -π/2. So the result is -π/2. 

But let's check with a simple numerical approximation. Let's approximate the integral using the midpoint rule with a few intervals. For example, take a few points between 0 and π/2. Let's take x = π/4, as before, the integrand is -ln 2 ≈ -0.6931. Let's take x = π/6: integrand is ln(1/2)/cos²(π/6) = (-ln 2)/( (√3/2)^2 ) = (-ln 2)/(3/4) = - (4/3) ln 2 ≈ -1.8484. At x = π/3: sin(π/3) = √3/2, so ln(√3/2) = ln(√3) - ln 2 = (1/2) ln 3 - ln 2 ≈ 0.5493 - 0.6931 = -0.1438. cos²(π/3) = (1/2)^2 = 1/4. So integrand is (-0.1438)/0.25 ≈ -0.5752. 

If we approximate the integral using these three points (midpoints between 0, π/6, π/3, π/2), but maybe this is too crude. Alternatively, use Simpson's rule with a few intervals. Let's try Simpson's 1/3 rule with two intervals (n=2). The interval from 0 to π/2 is divided into two intervals: h = (π/2)/2 = π/4. The points are x0=0, x1=π/4, x2=π/2. Simpson's rule formula is (h/3)[f(x0) + 4f(x1) + f(x2)]. But at x0=0, the integrand is ln(0)/1, which is -infty. Similarly, at x2=π/2, the integrand is 0/0, which is undefined. So Simpson's rule might not work here due to the singularities at the endpoints. 

Alternatively, use substitution to handle the singularities. Let me try substitution t = x near 0. Let x = t, as t approaches 0, the integrand behaves like ln t / 1, so integrating ln t from 0 to a small ε gives t ln t - t, which is finite. Similarly, near π/2, let x = π/2 - t, then the integrand behaves like ln(cos t)/sin²t ≈ (-t²/2)/t² = -1/2, so the integral near π/2 is approximately -1/2 * t, which is finite. So the integral is convergent. 

But how to approximate it numerically? Let's use a numerical integration method that can handle the singularities. Let's split the integral into two parts: from 0 to π/4 and π/4 to π/2. For the first part, from 0 to π/4, let's use substitution t = x, and for the integral from π/4 to π/2, use substitution t = π/2 - x. 

Alternatively, use adaptive quadrature. But since I'm doing this manually, let's approximate with a few points. Let's take x = π/6, π/4, π/3. Let's compute the integrand at these points:

At x=π/6: integrand ≈ -1.8484

At x=π/4: integrand ≈ -0.6931

At x=π/3: integrand ≈ -0.5752

If I take a rough average of these values and multiply by the interval π/2, but this is very approximate. Alternatively, use trapezoidal rule with a few intervals. Let's try from π/6 to π/3. But this is getting too helpful. Alternatively, use the analytical result. Since the analytical result is -π/2 ≈ -1.5708. Let's check if this makes sense. 

If the integrand is negative throughout, the integral should be negative. The value -1.5708 is approximately -π/2. Let's see if this matches with some known integrals. Wait, I recall that ∫₀^{π/2} ln(sin x) dx = - (π/2) ln 2. But that's a different integral. In our case, the integral is ln(sin x)/cos²x dx, which is different. 

Alternatively, maybe there's another approach. Let's consider substitution. Let t = tan x. Then dt/dx = sec²x = 1 + tan²x. So dx = dt / (1 + t²). Then the integral becomes ∫₀^{∞} [ln(t / sqrt(1 + t²))] / (1 / (1 + t²)) * (dt / (1 + t²)). Wait, this is similar to what I did before. Let's compute it again. 

sin x = t / sqrt(1 + t²), cos x = 1 / sqrt(1 + t²). So ln(sin x) = ln t - (1/2) ln(1 + t²). The denominator cos²x is 1/(1 + t²). So the integrand becomes [ln t - (1/2) ln(1 + t²)] / (1/(1 + t²)) * dx. But dx = dt / (1 + t²). So the integrand becomes [ln t - (1/2) ln(1 + t²)] * (1 + t²) * (dt / (1 + t²)) = [ln t - (1/2) ln(1 + t²)] dt. So the integral is ∫₀^∞ [ln t - (1/2) ln(1 + t²)] dt. 

Now, split this into two integrals: I1 = ∫₀^∞ ln t dt and I2 = ∫₀^∞ ln(1 + t²) dt. Then the integral is I1 - (1/2) I2. But both I1 and I2 are divergent. However, perhaps their combination is convergent. Let's compute I1 - (1/2) I2. 

Compute I1: ∫₀^∞ ln t dt. This diverges as t approaches infinity. Similarly, I2: ∫₀^∞ ln(1 + t²) dt also diverges. But maybe their combination converges. Let's consider integrating from 0 to A and then take A to infinity. 

Compute ∫₀^A [ln t - (1/2) ln(1 + t²)] dt. Integrate term by term:

∫ ln t dt = t ln t - t

∫ ln(1 + t²) dt. Let's integrate by parts. Let u = ln(1 + t²), dv = dt. Then du = (2t)/(1 + t²) dt, v = t. So ∫ ln(1 + t²) dt = t ln(1 + t²) - ∫ 2t²/(1 + t²) dt = t ln(1 + t²) - 2 ∫ [1 - 1/(1 + t²)] dt = t ln(1 + t²) - 2t + 2 arctan t.

So combining these:

The integral from 0 to A is [t ln t - t] - (1/2)[t ln(1 + t²) - 2t + 2 arctan t] evaluated from 0 to A.

At A:

= [A ln A - A] - (1/2)[A ln(1 + A²) - 2A + 2 arctan A]

At 0:

= [0 - 0] - (1/2)[0 - 0 + 0] = 0.

So the integral up to A is:

A ln A - A - (1/2)A ln(1 + A²) + A - arctan A

Simplify:

A ln A - (1/2) A ln(1 + A²) - arctan A

Now, let's analyze the limit as A approaches infinity.

First, A ln A - (1/2) A ln(1 + A²). Let's factor out A:

A [ln A - (1/2) ln(1 + A²)].

Note that ln(1 + A²) = ln(A²(1 + 1/A²)) = 2 ln A + ln(1 + 1/A²). So:

ln A - (1/2)(2 ln A + ln(1 + 1/A²)) = ln A - ln A + (1/2) ln(1 + 1/A²)) = (1/2) ln(1 + 1/A²) ≈ (1/2)(1/A²) for large A.

So the term becomes A * (1/(2A²)) = 1/(2A), which approaches 0 as A approaches infinity.

Then the remaining term is - arctan A. As A approaches infinity, arctan A approaches π/2. So the limit is -π/2. 

Therefore, the integral ∫₀^∞ [ln t - (1/2) ln(1 + t²)] dt = -π/2, which matches our previous analytical result. So the original integral is indeed -π/2. 

Therefore, the exact answer is -π/2. The numerical approximation is approximately -1.5707963268. Rounded to 10 decimal places, that's -1.5707963268. 

So the final answer should be {"answer": "-\\frac{\\pi}{2}", "numerical_answer": "-1.5707963268"}.
</think>

{"answer": "-\\frac{\\pi}{2}", "numerical_answer": "-1.5707963268"}