

To solve the definite integral \(\int_0^1 \frac{\ln(1+x+x^2)}{x} \, dx\), we proceed as follows:

### Step 1: Simplify the logarithm argument
Notice that \(1 + x + x^2 = \frac{1 - x^3}{1 - x}\) for \(x \neq 1\). Taking the natural logarithm of both sides gives:
\[
\ln(1 + x + x^2) = \ln\left(\frac{1 - x^3}{1 - x}\right) = \ln(1 - x^3) - \ln(1 - x).
\]

### Step 2: Rewrite the integral
Substituting this into the original integral, we split it into two parts:
\[
\int_0^1 \frac{\ln(1+x+x^2)}{x} \, dx = \int_0^1 \frac{\ln(1 - x^3)}{x} \, dx - \int_0^1 \frac{\ln(1 - x)}{x} \, dx.
\]

### Step 3: Evaluate the integrals using the dilogarithm function
The integral \(\int_0^z \frac{\ln(1 - t)}{t} \, dt\) is related to the dilogarithm function \(\text{Li}_2(z)\), defined as \(\text{Li}_2(z) = -\int_0^z \frac{\ln(1 - t)}{t} \, dt\). 

- For the second integral, \(\int_0^1 \frac{\ln(1 - x)}{x} \, dx = -\text{Li}_2(1)\). It is known that \(\text{Li}_2(1) = \frac{\pi^2}{6}\), so this integral equals \(-\frac{\pi^2}{6}\).

- For the first integral, substitute \(t = x^3\) (so \(x = t^{1/3}\) and \(dx = \frac{1}{3} t^{-2/3} dt\)). The integral becomes:
  \[
  \int_0^1 \frac{\ln(1 - x^3)}{x} \, dx = \int_0^1 \frac{\ln(1 - t)}{t^{1/3}} \cdot \frac{1}{3} t^{-2/3} \, dt = \frac{1}{3} \int_0^1 \frac{\ln(1 - t)}{t} \, dt = \frac{1}{3} (-\text{Li}_2(1)) = -\frac{\pi^2}{18}.
  \]

### Step 4: Combine the results
Subtracting the two integrals:
\[
\int_0^1 \frac{\ln(1+x+x^2)}{x} \, dx = \left(-\frac{\pi^2}{18}\right) - \left(-\frac{\pi^2}{6}\right) = \frac{\pi^2}{9}.
\]

### Numerical Approximation
Using \(\pi \approx 3.141592653589793\), we find \(\pi^2 \approx 9.869604401089358\). Thus:
\[
\frac{\pi^2}{9} \approx \frac{9.869604401089358}{9} \approx 1.0966227112.
\]

{"answer": "\(\frac{\pi^2}{9}\)", "numerical_answer": "1.0966227112"}