<think>
Okay, let's see. I need to compute the definite integral of x squared times the cube root of (x cubed plus 1) from -1 to 1. Hmm. Alright, step by step.

First, the integral is ∫ from -1 to 1 of x² * ∛(x³ + 1) dx. Let me try to simplify this. The cube root is the same as raising to the 1/3 power, so maybe I can help. Let me think about substitution. The inside of the cube root is x³ + 1. If I let u be x³ + 1, then du/dx is 3x². Oh, wait, there's an x² in the integrand. That seems promising. Let's try that substitution.

Let u = x³ + 1. Then du = 3x² dx. So, (1/3) du = x² dx. That's perfect because the integrand has x² dx multiplied by the cube root of u. So substituting, the integral becomes (1/3) ∫ ∛u du. But wait, I need to adjust the limits of integration when I substitute. When x is -1, u = (-1)^3 + 1 = -1 + 1 = 0. When x is 1, u = 1^3 + 1 = 2. So the integral becomes from u=0 to u=2.

So now, the integral is (1/3) ∫ from 0 to 2 of u^(1/3) du. Integrating u^(1/3) is straightforward. The integral of u^(n) is u^(n+1)/(n+1) as long as n ≠ -1. Here, n = 1/3, so n+1 = 4/3. Therefore, the integral becomes (1/3) * [ (u^(4/3))/(4/3) ) ] evaluated from 0 to 2. Simplify that expression.

Multiplying (1/3) by (3/4) gives 1/4. So the integral is (1/4) [ u^(4/3) ] from 0 to 2. Plugging in the limits: (1/4)(2^(4/3) - 0^(4/3)). Since 0^(4/3) is 0, this simplifies to (1/4) * 2^(4/3).

Now, 2^(4/3) can be written as (2^(1/3))^4, which is the cube root of 2 raised to the 4th power. Alternatively, 2^(4/3) is 2^(1 + 1/3) = 2 * 2^(1/3). So, 2^(4/3) = 2 * 2^(1/3). Therefore, the exact value is (1/4) * 2 * 2^(1/3) = (1/2) * 2^(1/3). Alternatively, 2^(1/3)/2. But maybe it's better to write it as (2^(4/3))/4. Either way is correct.

Alternatively, 2^(4/3) is 2^(1 + 1/3) = 2 * 2^(1/3), so (2 * 2^(1/3))/4 = (2^(1/3))/2. So the exact answer is 2^(1/3)/2. Wait, let me check that again. Let's compute 2^(4/3) divided by 4. 2^(4/3) is 2^(1 + 1/3) = 2 * 2^(1/3). So 2 * 2^(1/3) divided by 4 is (2^(1/3))/2. So yes, the exact answer is 2^(1/3)/2. Alternatively, in fractional exponent terms, 2^(1/3) is 2^{1/3}, so 2^{1/3}/2 is the same as 2^{-2/3}. Wait, 2^{1/3}/2 = 2^{1/3 - 1} = 2^{-2/3} = 1/(2^{2/3}). But both forms are correct. Which one is simpler? Maybe 2^{1/3}/2 is more straightforward.

But let me confirm the substitution steps again to make sure I didn't make a mistake. The substitution was u = x³ +1, du = 3x² dx, so x² dx = du/3. The limits when x=-1: u=0, x=1: u=2. The integrand becomes u^{1/3} * (du/3). So integrating from 0 to 2, (1/3) ∫u^{1/3} du. The integral of u^{1/3} is (u^{4/3})/(4/3) = (3/4)u^{4/3}. Multiply by 1/3: (1/3)*(3/4) = 1/4. Then [u^{4/3}/4] from 0 to 2. So 2^{4/3}/4 - 0 = 2^{4/3}/4. Which is the same as 2^{4/3 - 2} because 4 is 2^2. Wait, 2^{4/3}/4 = 2^{4/3}/2^2 = 2^{4/3 - 2} = 2^{-2/3} = 1/(2^{2/3}). Alternatively, 2^{4/3} is 2^(1 + 1/3) = 2 * 2^(1/3), so 2 * 2^(1/3)/4 = 2^(1/3)/2. So both forms are equivalent. So the exact answer can be written as \frac{\sqrt[3]{2}}{2} or \frac{2^{1/3}}{2} or 2^{-2/3}. But perhaps the first form is more intuitive.

Now, for the numerical approximation. Let's compute 2^(1/3). The cube root of 2 is approximately 1.259921049894873. Then divide by 2: 1.259921049894873 / 2 ≈ 0.6299605249. Rounded to 10 decimal places, that's 0.6299605249. Let me check with a calculator. 2^(1/3) ≈ 1.2599210498948732, so half of that is approximately 0.6299605249474366. So rounding to 10 decimal places would be 0.6299605249. Wait, but let me verify with more precise calculation. Let me use a calculator. Alternatively, 2^(1/3) is approximately 1.2599210498948731648, so dividing by 2 gives 0.6299605249474365824. So up to 10 decimal places, that's 0.6299605249. So the numerical approximation is 0.6299605249.

Wait, let me check if the integral is correct. Let me think again. The substitution is correct? Let me check with x from -1 to 1. The function x² * cube root(x³ +1). But when x is negative, x³ is negative. For example, when x is -1, x³ +1 is 0. So the cube root is defined here. The integrand is x² times cube root(x³ +1). Since x² is always non-negative, and cube root is defined for all real numbers, including negative ones. So the integrand is real and continuous over [-1,1]. So the substitution should be valid. Also, the substitution u = x³ +1 works here. The substitution is valid because the derivative 3x² is present except at x=0, but since x² is non-negative, and the interval is from -1 to 1, which includes x=0, but the substitution is still valid because the function is smooth here. So the substitution is okay.

Another way to verify the integral from -1 to 1 of x² * (x³ +1)^(1/3) dx. Let me check if the antiderivative is correct. The substitution gives us (1/4)u^(4/3) evaluated from 0 to 2, which is (1/4)(2^(4/3) - 0) = 2^(4/3)/4. Which is the same as 2^(4/3 - 2) = 2^(-2/3) = 1/(2^(2/3)). Alternatively, 2^(4/3) is 2^(1 + 1/3) = 2 * 2^(1/3), so 2*2^(1/3)/4 = 2^(1/3)/2. So both forms are equivalent. So the exact answer is 2^(1/3)/2, which is the same as 2^{-2/3}. Either form is acceptable, but perhaps writing it as \frac{\sqrt[3]{2}}{2} is more straightforward in LaTeX.

Therefore, the exact answer is \frac{\sqrt[3]{2}}{2} and the numerical approximation is approximately 0.6299605249.
</think>

{"answer": "\\frac{\\sqrt[3]{2}}{2}", "numerical_answer": 0.6299605249}