We start with the integral

  I = ∫₀^π cos(x + cos x) dx.

Step 1. Change of variable by symmetry:
Let t = π − x. Then when x = 0 we have t = π, and when x = π we have t = 0. Also, dx = −dt. Changing the variable, the integral becomes

  I = ∫₀^π cos(x + cos x) dx 
    = ∫ₚ⁰ cos((π − t) + cos(π − t)) (−dt)
    = ∫₀^π cos((π − t) + cos(π − t)) dt.

Now, recall that cos(π − t) = − cos t, so
  cos((π − t) + cos(π − t)) = cos((π − t) − cos t).

Step 2. Use the cosine identity:
Using the identity cos(π − θ) = − cos θ for any angle θ, set θ = t + cos t. Then
  cos((π − t) − cos t) = cos(π − (t + cos t)) = − cos(t + cos t).

Thus, the integral now reads

  I = ∫₀^π [− cos(t + cos t)] dt = − ∫₀^π cos(t + cos t) dt.

But note that if we rename the dummy variable t back as x, this is the same as

  I = − I.

Step 3. Conclude:
We have I = − I, which implies that 2I = 0, so

  I = 0.

Step 4. Numerical approximation:
The numerical value is 0.0000000000 when rounded to ten decimal places.

Final Answer in JSON format:
{"answer": "$0$", "numerical_answer": "0.0000000000"}