# Evaluating $\int\limits_{0}^{2}x^{-1/2}(2-x)^{-1/2}\cosh\left(\sqrt{x(2-x)}\right)dx$

I'll solve this definite integral by making an appropriate substitution.

## Step 1: Substitution
Let's set $x = 1 - \cos(\theta)$ or $x = 1 + \cos(\theta)$. Actually, let's try $x = 1 - \cos(\theta)$ first.

This gives:
- $x = 1 - \cos(\theta)$
- $dx = \sin(\theta) d\theta$
- When $x = 0$, $\cos(\theta) = 1$, so $\theta = 0$
- When $x = 2$, $\cos(\theta) = -1$, so $\theta = \pi$

Let's compute the other terms:
- $2-x = 2-(1-\cos(\theta)) = 1+\cos(\theta)$
- $\sqrt{x(2-x)} = \sqrt{(1-\cos(\theta))(1+\cos(\theta))} = \sqrt{1-\cos^2(\theta)} = \sqrt{\sin^2(\theta)} = \sin(\theta)$ (since $\sin(\theta) \geq 0$ in $[0,\pi]$)

So we have:
- $x^{-1/2} = (1-\cos(\theta))^{-1/2}$
- $(2-x)^{-1/2} = (1+\cos(\theta))^{-1/2}$
- $\cosh(\sqrt{x(2-x)}) = \cosh(\sin(\theta))$

## Step 2: Rewriting the integral
The integral becomes:
$$\int_{0}^{\pi} (1-\cos(\theta))^{-1/2} (1+\cos(\theta))^{-1/2} \cosh(\sin(\theta)) \sin(\theta) d\theta$$

We can simplify $(1-\cos(\theta))^{-1/2} (1+\cos(\theta))^{-1/2}$:

$$(1-\cos(\theta))^{-1/2} (1+\cos(\theta))^{-1/2} = \frac{1}{\sqrt{1-\cos^2(\theta)}} = \frac{1}{\sin(\theta)}$$

Since $\sin(\theta) > 0$ in $(0,\pi)$, our integral becomes:
$$\int_{0}^{\pi} \frac{1}{\sin(\theta)} \cosh(\sin(\theta)) \sin(\theta) d\theta = \int_{0}^{\pi} \cosh(\sin(\theta)) d\theta$$

## Step 3: Using symmetry
Since $\sin(\pi-\theta) = \sin(\theta)$ and $\cosh$ is an even function, the integrand $\cosh(\sin(\theta))$ is symmetric around $\theta = \pi/2$. So:

$$\int_{0}^{\pi} \cosh(\sin(\theta)) d\theta = 2\int_{0}^{\pi/2} \cosh(\sin(\theta)) d\theta$$

## Step 4: Using the definition of hyperbolic cosine
$\cosh(x) = \frac{e^x + e^{-x}}{2}$, so:
$$\int_{0}^{\pi/2} \cosh(\sin(\theta)) d\theta = \int_{0}^{\pi/2} \frac{e^{\sin(\theta)} + e^{-\sin(\theta)}}{2} d\theta$$

The integral $\int_{0}^{\pi/2} e^{\sin(\theta)} d\theta$ equals $\int_{0}^{\pi/2} e^{-\sin(\theta)} d\theta$ by substituting $\theta' = \pi-\theta$.

Therefore:
$$2\int_{0}^{\pi/2} \cosh(\sin(\theta)) d\theta = 2\int_{0}^{\pi/2} \frac{e^{\sin(\theta)} + e^{-\sin(\theta)}}{2} d\theta = 2\int_{0}^{\pi/2} e^{\sin(\theta)} d\theta$$

## Step 5: Recognizing the modified Bessel function
The integral $\int_{0}^{\pi/2} e^{\sin(\theta)} d\theta = \frac{\pi}{2}I_0(1)$, where $I_0$ is the modified Bessel function of the first kind of order 0.

## Step 6: Final result
Our original integral equals $\pi I_0(1)$.

## Numerical approximation
The value of $I_0(1) \approx 1.2660658777520084$, so:
$\pi I_0(1) \approx 3.9789527279189754$

Therefore, to 10 decimal places: $3.9789527279$

{"answer": "\pi I_0(1)", "numerical_answer": "3.9789527279"}