Let's solve the integral step by step:

\[
I = \int_0^1 \sin^2(\log x) \, dx
\]

**Step 1: Express \(\sin^2(\log x)\) using a double-angle identity.**

Recall,
\[
\sin^2\theta = \frac{1 - \cos(2\theta)}{2}
\]

So,
\[
I = \int_0^1 \frac{1 - \cos(2\log x)}{2} \, dx
= \frac{1}{2} \int_0^1 1 \, dx - \frac{1}{2} \int_0^1 \cos(2\log x) \, dx
\]

The first term:
\[
\frac{1}{2} \int_0^1 1 \, dx = \frac{1}{2} (1-0) = \frac{1}{2}
\]

Now for the second term,
\[
I_2 = \int_0^1 \cos(2\log x) \, dx
\]

**Step 2: Make the substitution \( x = e^t \), \( dx = e^t dt \), as \( x \) goes from 0 to 1, \( t \) goes from \( -\infty \) to 0.**

So,
\[
I_2 = \int_{t=-\infty}^0 \cos(2t) \cdot e^t dt
\]

We can generally write,
\[
\int \cos(a t) \cdot e^{b t} dt = \frac{e^{b t}}{a^2 + b^2} (b \cos(a t) + a \sin(a t)) + C
\]

Here, \( a = 2, \ b = 1 \):

So,
\[
I_2 = \left[ \frac{e^t}{2^2 + 1^2} (1 \cdot \cos 2t + 2 \cdot \sin 2t) \right]_{-\infty}^0
= \left[ \frac{e^t ( \cos 2t + 2 \sin 2t )}{5} \right]_{-\infty}^0
\]

Evaluate at \( t = 0 \):
\[
e^0 ( \cos 0 + 2 \sin 0 ) = 1 (1 + 0) = 1
\]
So numerator is 1, denominator is 5: value is \( \frac{1}{5} \).

At \( t \to -\infty \):
\[
e^{t} \to 0,
\]
and the numerator is bounded, so the expression goes to 0.

Total:
\[
I_2 = \frac{1}{5} - 0 = \frac{1}{5}
\]

**Step 3: Put it all together**

Recall:
\[
I = \frac{1}{2} - \frac{1}{2} \left( \frac{1}{5} \right) = \frac{1}{2} - \frac{1}{10} = \frac{4}{10} = \frac{2}{5}
\]

**Step 4: Numerical Approximation**

\[
\frac{2}{5} = 0.4
\]

Rounded to 10 decimal places: \( 0.4000000000 \)

---

Final answer in the required format:

{"answer": "\\frac{2}{5}", "numerical_answer": "0.4000000000"}