

To solve the definite integral \(\int_1^3 \frac{\ln(x)}{x^2 + 3} \, dx\), we proceed as follows:

### Step 1: Integration by Parts
Let \( u = \ln(x) \) and \( dv = \frac{1}{x^2 + 3} \, dx \). Then:
- \( du = \frac{1}{x} \, dx \)
- \( v = \frac{1}{\sqrt{3}} \arctan\left(\frac{x}{\sqrt{3}}\right) \) (since \( \int \frac{1}{x^2 + a^2} \, dx = \frac{1}{a} \arctan\left(\frac{x}{a}\right) + C \) with \( a = \sqrt{3} \))

By integration by parts (\(\int u \, dv = uv - \int v \, du\)):
\[
\int_1^3 \frac{\ln(x)}{x^2 + 3} \, dx = \left[ \ln(x) \cdot \frac{1}{\sqrt{3}} \arctan\left(\frac{x}{\sqrt{3}}\right) \right]_1^3 - \int_1^3 \frac{1}{\sqrt{3}} \arctan\left(\frac{x}{\sqrt{3}}\right) \cdot \frac{1}{x} \, dx
\]

### Step 2: Evaluate the Boundary Term
The first term evaluates to:
\[
\left[ \ln(3) \cdot \frac{1}{\sqrt{3}} \arctan\left(\frac{3}{\sqrt{3}}\right) - \ln(1) \cdot \frac{1}{\sqrt{3}} \arctan\left(\frac{1}{\sqrt{3}}\right) \right]
\]
Since \( \ln(1) = 0 \) and \( \arctan\left(\sqrt{3}\right) = \frac{\pi}{3} \), this simplifies to:
\[
\frac{\ln(3)}{\sqrt{3}} \cdot \frac{\pi}{3} = \frac{\pi \ln(3)}{3\sqrt{3}}
\]

### Step 3: Simplify the Remaining Integral
The remaining integral is:
\[
- \frac{1}{\sqrt{3}} \int_1^3 \frac{\arctan\left(\frac{x}{\sqrt{3}}\right)}{x} \, dx
\]
Let \( t = \frac{x}{\sqrt{3}} \), so \( x = t\sqrt{3} \) and \( dx = \sqrt{3} \, dt \). The limits change from \( x=1 \) to \( t=\frac{1}{\sqrt{3}} \) and \( x=3 \) to \( t=\sqrt{3} \). The integral becomes:
\[
- \frac{1}{\sqrt{3}} \int_{\frac{1}{\sqrt{3}}}^{\sqrt{3}} \frac{\arctan(t)}{t} \, dt
\]

### Step 4: Evaluate \( \int_{\frac{1}{\sqrt{3}}}^{\sqrt{3}} \frac{\arctan(t)}{t} \, dt \)
Using the identity \( \arctan(t) = \frac{\pi}{2} - \arctan\left(\frac{1}{t}\right) \) for \( t > 0 \), split the integral at \( t=1 \):
\[
\int_{\frac{1}{\sqrt{3}}}^{\sqrt{3}} \frac{\arctan(t)}{t} \, dt = \int_{\frac{1}{\sqrt{3}}}^1 \frac{\arctan(t)}{t} \, dt + \int_1^{\sqrt{3}} \left( \frac{\pi}{2t} - \frac{\arctan\left(\frac{1}{t}\right)}{t} \right) dt
\]
The second integral simplifies using \( u = \frac{1}{t} \), leading to cancellation of the \( \arctan(t)/t \) terms. The result is:
\[
\int_{\frac{1}{\sqrt{3}}}^{\sqrt{3}} \frac{\arctan(t)}{t} \, dt = \frac{\pi \ln(3)}{4}
\]

### Step 5: Combine Results
Substituting back, the original integral becomes:
\[
\frac{\pi \ln(3)}{3\sqrt{3}} - \frac{1}{\sqrt{3}} \cdot \frac{\pi \ln(3)}{4} = \frac{\pi \ln(3)}{12\sqrt{3}} = \frac{\pi \sqrt{3} \ln(3)}{36}
\]

### Numerical Approximation
Using \( \pi \approx 3.1415926535 \), \( \sqrt{3} \approx 1.7320508076 \), and \( \ln(3) \approx 1.0986122887 \):
\[
\frac{\pi \sqrt{3} \ln(3)}{36} \approx \frac{3.1415926535 \cdot 1.7320508076 \cdot 1.0986122887}{36} \approx 0.1660551651
\]

{"answer": "\\frac{\\pi \\sqrt{3} \\ln 3}{36}", "numerical_answer": "0.1660551651"}