To solve the definite integral 
\[
\int_0^1 \frac{e^{\arctan(x)}}{(x^2 + 1)^{3/2}} \, dx,
\]
we will follow these steps:

### Step 1: Substitution
Letâ€™s make the substitution:
\[
u = \arctan(x).
\]
Then, the derivative of \( u \) with respect to \( x \) is:
\[
\frac{du}{dx} = \frac{1}{x^2 + 1} \quad \Rightarrow \quad dx = (x^2 + 1) \, du.
\]
When \( x = 0 \), \( u = 0 \), and when \( x = 1 \), \( u = \frac{\pi}{4} \).

The integral becomes:
\[
\int_{0}^{\frac{\pi}{4}} \frac{e^u}{(x^2 + 1)^{3/2}} \cdot (x^2 + 1) \, du = \int_{0}^{\frac{\pi}{4}} \frac{e^u}{(x^2 + 1)^{1/2}} \, du.
\]
However, we need to express \( x^2 + 1 \) in terms of \( u \). Since \( x = \tan(u) \), we have:
\[
x^2 + 1 = \tan^2(u) + 1 = \sec^2(u).
\]
Thus, the integral simplifies to:
\[
\int_{0}^{\frac{\pi}{4}} \frac{e^u}{\sec(u)} \, du = \int_{0}^{\frac{\pi}{4}} e^u \cos(u) \, du.
\]

### Step 2: Integration by Parts
To evaluate \( \int e^u \cos(u) \, du \), we use integration by parts. Let:
\[
I = \int e^u \cos(u) \, du.
\]
Let \( v = e^u \), \( dw = \cos(u) \, du \). Then \( dv = e^u \, du \), \( w = \sin(u) \). Applying integration by parts:
\[
I = e^u \sin(u) - \int e^u \sin(u) \, du.
\]
Now, apply integration by parts again to \( \int e^u \sin(u) \, du \). Let \( v = e^u \), \( dw = \sin(u) \, du \). Then \( dv = e^u \, du \), \( w = -\cos(u) \):
\[
\int e^u \sin(u) \, du = -e^u \cos(u) + \int e^u \cos(u) \, du = -e^u \cos(u) + I.
\]
Substituting back:
\[
I = e^u \sin(u) - (-e^u \cos(u) + I) = e^u \sin(u) + e^u \cos(u) - I.
\]
Solving for \( I \):
\[
2I = e^u (\sin(u) + \cos(u)) \quad \Rightarrow \quad I = \frac{e^u (\sin(u) + \cos(u))}{2}.
\]

### Step 3: Evaluate the Definite Integral
Now, evaluate \( I \) from \( 0 \) to \( \frac{\pi}{4} \):
\[
\left. \frac{e^u (\sin(u) + \cos(u))}{2} \right|_{0}^{\frac{\pi}{4}} = \frac{e^{\frac{\pi}{4}} \left( \sin\left(\frac{\pi}{4}\right) + \cos\left(\frac{\pi}{4}\right) \right)}{2} - \frac{e^0 (\sin(0) + \cos(0))}{2}.
\]
Simplify:
\[
\sin\left(\frac{\pi}{4}\right) = \cos\left(\frac{\pi}{4}\right) = \frac{\sqrt{2}}{2}, \quad \sin(0) = 0, \quad \cos(0) = 1.
\]
Thus:
\[
\frac{e^{\frac{\pi}{4}} \left( \frac{\sqrt{2}}{2} + \frac{\sqrt{2}}{2} \right)}{2} - \frac{1 \cdot (0 + 1)}{2} = \frac{e^{\frac{\pi}{4}} \sqrt{2}}{2} - \frac{1}{2}.
\]

### Step 4: Final Answer
The exact value of the integral is:
\[
\frac{e^{\frac{\pi}{4}} \sqrt{2} - 1}{2}.
\]
A numerical approximation to 10 decimal places is:
\[
0.7450780724.
\]

### JSON Output
```json
{"answer": "\\frac{e^{\\frac{\\pi}{4}} \\sqrt{2} - 1}{2}", "numerical_answer": "0.7450780724"}
```