Let's compute the definite integral
\[
I = \int_{-1}^1 \frac{\cos x}{1 + e^{-\frac{1}{x}}}\,dx.
\]

Let's proceed step by step:

**Step 1: Analyze the integrand and attempt a substitution or symmetry.**

Let’s try to relate the values at \( x \) and \( -x \):

Let \( f(x) = \frac{\cos x}{1 + e^{-1/x}} \).

Consider the transformation \( x \to -x \):

\[
f(-x) = \frac{\cos(-x)}{1 + e^{-1/(-x)}} = \frac{\cos x}{1 + e^{1/x}}
\]

So,

\[
f(x) + f(-x) = \frac{\cos x}{1 + e^{-1/x}} + \frac{\cos x}{1 + e^{1/x}}
\]

Let’s combine these:

\[
= \cos x \left( \frac{1}{1 + e^{-1/x}} + \frac{1}{1 + e^{1/x}} \right)
\]

Find a common denominator:

The denominators are \( (1 + e^{-1/x})(1 + e^{1/x}) \).

Calculate sum:

\[
\frac{1}{1 + e^{-1/x}} + \frac{1}{1 + e^{1/x}}
= \frac{(1 + e^{1/x}) + (1 + e^{-1/x})}{(1 + e^{-1/x})(1 + e^{1/x})}
= \frac{2 + e^{1/x} + e^{-1/x}}{(1 + e^{-1/x})(1 + e^{1/x})}
\]

Now, expand denominator:

\[
(1 + e^{-1/x})(1 + e^{1/x}) = 1 + e^{-1/x} + e^{1/x} + e^{-1/x}e^{1/x}
\]
But \( e^{-1/x}e^{1/x} = e^0 = 1 \), so

\[
= 1 + e^{-1/x} + e^{1/x} + 1 = 2 + e^{-1/x} + e^{1/x}
\]

So numerator and denominator are equal:

\[
f(x) + f(-x) = \cos x \cdot \frac{2 + e^{1/x} + e^{-1/x}}{2 + e^{-1/x} + e^{1/x}} = \cos x \cdot 1 = \cos x
\]

So,

\[
f(x) + f(-x) = \cos x
\]

**Step 2: Use symmetry to evaluate the integral.**

So,

\[
I = \int_{-1}^1 f(x)\,dx = \int_{-1}^1 \frac{\cos x}{1 + e^{-1/x}}\,dx
\]
But over \([-1,1]\):

\[
I = \int_{-1}^1 f(x)\,dx = \frac{1}{2}\int_{-1}^1 (f(x) + f(-x))\,dx = \frac{1}{2}\int_{-1}^1 \cos x\,dx
\]

**Step 3: Integrate \(\cos x\) from \(-1\) to \(1\):**

\[
\int_{-1}^1 \cos x\,dx = [\sin x]_{-1}^1 = \sin 1 - \sin(-1) = \sin 1 + \sin 1 = 2\sin 1
\]

Thus,

\[
I = \frac{1}{2} \times 2\sin 1 = \sin 1
\]

**Step 4: Numerical approximation**

\[
\sin 1 \approx 0.8414709848
\]

---

**Final Answer:**

```json
{"answer": "\\sin 1", "numerical_answer": "0.8414709848"}
```