<think>
Okay, let's tackle this integral step by step. The integral given is ∫₀² x^(1.0 - 3/2) (2.0 - x)^(1.0 - 1/2) [1 - 0.5x(2.0 - x)]^(-1.0) dx. First, I need to simplify the exponents and the integrand. 

Starting with the exponents: 1.0 - 3/2 is equal to -1/2, and 1.0 - 1/2 is 1/2. So the integral becomes ∫₀² x^(-1/2) (2 - x)^(1/2) [1 - 0.5x(2 - x)]^(-1) dx. Let me check that again. Yes, 1.0 minus 3/2 is indeed -1/2, and 1.0 minus 1/2 is 1/2. So the integrand simplifies to x^(-1/2) times (2 - x)^(1/2) divided by [1 - 0.5x(2 - x)].

Next, let's simplify the denominator inside the brackets. The term 0.5x(2 - x) can be expanded. Let's compute that: 0.5x*(2 - x) = x - 0.5x². Therefore, 1 - 0.5x(2 - x) becomes 1 - x + 0.5x². Wait, that's 1 - x + 0.5x². Hmm, maybe there's a way to write this as a quadratic expression. Let me check: 0.5x² - x + 1. Let's factor out 0.5: 0.5(x² - 2x + 2). But I don't know if that helps. Alternatively, maybe completing the square. Let's see: x² - 2x + 2 = (x - 1)^2 + 1. So 0.5[(x - 1)^2 + 1]. Not sure if that's useful yet.

So the integrand is x^(-1/2) (2 - x)^(1/2) divided by [1 - x + 0.5x²]. Let me write that as x^{-1/2} (2 - x)^{1/2} / (0.5x² - x + 1). Hmm. Maybe there's a substitution that can help here. Let's consider substitution to simplify the integral.

Alternatively, perhaps this integral is related to the Beta function or the Gamma function. The presence of x^(-1/2) and (2 - x)^(1/2) suggests a Beta function form, but usually Beta functions are integrals from 0 to a of x^{c} (a - x)^d dx. However, the denominator complicates things. Let me recall that the Beta function is ∫₀¹ t^{c-1} (1 - t)^{d-1} dt = B(c, d) = Γ(c)Γ(d)/Γ(c + d). But here, the limits are from 0 to 2, and there's an extra term. Maybe a substitution to transform the interval to [0,1]?

Let me try substitution. Let t = x/2, so x = 2t, dx = 2dt. Then the limits when x=0, t=0; x=2, t=1. Substituting into the integral:

∫₀¹ (2t)^{-1/2} (2 - 2t)^{1/2} [1 - 0.5*(2t)(2 - 2t)]^{-1} * 2 dt.

Simplify each term:

(2t)^{-1/2} = (2)^{-1/2} t^{-1/2}

(2 - 2t)^{1/2} = (2(1 - t))^{1/2} = 2^{1/2} (1 - t)^{1/2}

The denominator: 1 - 0.5*(2t)(2 - 2t) = 1 - 0.5*(4t - 4t²) = 1 - 2t + 2t²

So putting it all together:

2^{-1/2} t^{-1/2} * 2^{1/2} (1 - t)^{1/2} / (1 - 2t + 2t²) * 2 dt

Simplify the constants: 2^{-1/2} * 2^{1/2} = 1, and then multiplied by 2 gives 2. So the integral becomes:

2 ∫₀¹ t^{-1/2} (1 - t)^{1/2} / (1 - 2t + 2t²) dt

Hmm, so now the integral is 2 ∫₀¹ t^{-1/2} (1 - t)^{1/2} / (2t² - 2t + 1) dt. Let me check the denominator again: 1 - 2t + 2t² is the same as 2t² - 2t + 1. Let's factor the denominator. The quadratic equation: 2t² - 2t + 1. The discriminant is (-2)^2 - 4*2*1 = 4 - 8 = -4, which is negative, so it doesn't factor into real roots. That complicates things. Maybe partial fractions won't work here. Alternatively, perhaps another substitution.

Alternatively, maybe we can express the denominator in terms of (t - a)^2 + b^2. Let's complete the square for 2t² - 2t + 1. Let's factor out 2: 2(t² - t) + 1. Then complete the square inside the parentheses: t² - t = t² - t + (1/4) - (1/4) = (t - 1/2)^2 - 1/4. So substituting back: 2[(t - 1/2)^2 - 1/4] + 1 = 2(t - 1/2)^2 - 1/2 + 1 = 2(t - 1/2)^2 + 1/2. So the denominator is 2(t - 1/2)^2 + 1/2. Hmm, which is 1/2*(4(t - 1/2)^2 + 1). Not sure if that helps.

Alternatively, maybe a trigonometric substitution. Let me see. Let u = t - 1/2, then the denominator becomes 2u² + 1/2. Let me check: 2(t - 1/2)^2 + 1/2 = 2u² + 1/2. So if we set u = (t - 1/2), then du = dt, and t = u + 1/2. The integral becomes from t=0 to t=1, so u ranges from -1/2 to 1/2. So the integral becomes:

2 ∫_{-1/2}^{1/2} (u + 1/2)^{-1/2} (1 - (u + 1/2))^{1/2} / (2u² + 1/2) du

Simplify the terms inside the integrand:

1 - (u + 1/2) = 1 - u - 1/2 = 1/2 - u. So (1/2 - u)^{1/2}

So the integrand is (u + 1/2)^{-1/2} (1/2 - u)^{1/2} / (2u² + 1/2)

Hmm, this seems more complex. Maybe not the best substitution. Let's think differently.

Alternatively, perhaps consider that the integrand after substitution is 2 ∫₀¹ t^{-1/2} (1 - t)^{1/2} / (2t² - 2t + 1) dt. Let me check if this can be expressed in terms of known integrals or if there's a substitution that can help. Let's look at the denominator 2t² - 2t + 1. Maybe write it as 2(t² - t) + 1. Let me try substitution z = t - 1/2, but similar to before. Alternatively, perhaps a substitution that can relate to Beta function.

Alternatively, maybe use hypergeometric functions, but the problem states to compute the integral analytically, so perhaps there's a closed-form solution. Let me check if the integrand can be expressed in terms of a Beta function times some factor. The presence of t^{-1/2} (1 - t)^{1/2} is similar to Beta function parameters. The Beta function B(a,b) is ∫₀¹ t^{a-1} (1 - t)^{b-1} dt. Here, a = 1/2, b = 3/2, since t^{-1/2} is t^{1/2 - 1} and (1 - t)^{1/2} is (1 - t)^{3/2 - 1}? Wait, no. Wait, the integrand here is t^{-1/2} (1 - t)^{1/2}, so that would be a = 1/2, b = 3/2. So B(1/2, 3/2) = Γ(1/2)Γ(3/2)/Γ(2) = (sqrt(π) * (sqrt(π)/2)) / 1! ) = π/2. But here, the denominator complicates things. If the denominator were a constant, then the integral would be straightforward. But since it's a function of t, perhaps we need to expand it as a series or find another approach.

Alternatively, maybe perform substitution to rationalize the denominator. Let me see. The denominator is 2t² - 2t + 1. Let me check if it can be written as (at + b)^2 + c^2. Let's see: 2t² - 2t + 1 = 2(t² - t) + 1. Completing the square inside the parentheses: t² - t = (t - 0.5)^2 - 0.25. So substituting back: 2[(t - 0.5)^2 - 0.25] + 1 = 2(t - 0.5)^2 - 0.5 + 1 = 2(t - 0.5)^2 + 0.5. So denominator is 2(t - 0.5)^2 + 0.5. Let me factor out 0.5: 0.5[4(t - 0.5)^2 + 1]. So denominator = 0.5[ (2(t - 0.5))^2 + 1 ]. Let me set u = 2(t - 0.5), then du = 2 dt, so dt = du/2. When t=0, u=2*(-0.5)= -1; when t=1, u=2*(0.5)=1. So the integral becomes:

2 ∫_{-1}^{1} [ ( (u/2 + 0.5) )^{-1/2} (1 - (u/2 + 0.5))^{1/2} / (0.5(u² + 1)) ) * (du/2) ]

Wait, let's substitute t = u/2 + 0.5, so u = 2(t - 0.5). Then t = (u + 1)/2. So substituting into the integrand:

t^{-1/2} = [(u + 1)/2]^{-1/2} = 2^{1/2} (u + 1)^{-1/2}

(1 - t)^{1/2} = [1 - (u + 1)/2]^{1/2} = [(1 - u)/2]^{1/2} = 2^{-1/2} (1 - u)^{1/2}

Denominator: 0.5(u² + 1) = (u² + 1)/2

Putting it all together:

2 * ∫_{-1}^{1} [2^{1/2} (u + 1)^{-1/2} * 2^{-1/2} (1 - u)^{1/2} / ( (u² + 1)/2 ) ] * (du/2)

Simplify the constants:

2^{1/2} * 2^{-1/2} = 1

Then, divided by (u² + 1)/2 is multiplied by 2/(u² + 1)

And multiplied by du/2.

So overall:

2 * [1 * 2/(u² + 1) * (u + 1)^{-1/2} (1 - u)^{1/2} ] * (du/2)

The 2 and the 1/2 cancel, leaving:

∫_{-1}^{1} (u + 1)^{-1/2} (1 - u)^{1/2} / (u² + 1) du

Hmm, this seems a bit simpler. Now, the integrand is (1 - u)^{1/2} (1 + u)^{-1/2} / (1 + u²). Let me write that as sqrt(1 - u)/sqrt(1 + u) / (1 + u²). Maybe another substitution. Let me consider substituting v = sqrt((1 - u)/(1 + u)). Let's try that. Let v = sqrt( (1 - u)/(1 + u) ). Then v² = (1 - u)/(1 + u). Solving for u: v²(1 + u) = 1 - u => v² + v² u = 1 - u => u(v² + 1) = 1 - v² => u = (1 - v²)/(1 + v²). Then du/dv = [ -2v(1 + v²) - (1 - v²)(2v) ] / (1 + v²)^2. Let me compute that:

Numerator: -2v(1 + v²) - (1 - v²)(2v) = -2v - 2v³ - 2v + 2v³ = -4v

So du = [ -4v / (1 + v²)^2 ] dv

Now, let's change the limits. When u = -1, v = sqrt( (1 - (-1))/(1 + (-1)) ) = sqrt(2/0), which is undefined. Wait, but u ranges from -1 to 1. When u approaches -1 from the right, (1 - u) approaches 2, and (1 + u) approaches 0, so v approaches infinity. When u = 1, v = 0. So the substitution might be from v = ∞ to v = 0. But this seems problematic. Maybe this substitution isn't the best approach. Let's try another substitution.

Alternatively, let's consider substituting u = sinθ. But the denominator is 1 + u², which would become 1 + sin²θ. Not sure. Alternatively, substitute u = tanφ. Let me try that. Let u = tanφ, so du = sec²φ dφ. Then 1 + u² = sec²φ. The limits when u = -1, φ = -π/4; when u = 1, φ = π/4. So the integral becomes:

∫_{-π/4}^{π/4} [sqrt(1 - tanφ) / sqrt(1 + tanφ) ] * [1 / sec²φ] * sec²φ dφ

Wait, the denominator 1 + u² is sec²φ, and du = sec²φ dφ, so the integral becomes:

∫ [sqrt(1 - tanφ)/sqrt(1 + tanφ)] * (1/sec²φ) * sec²φ dφ = ∫ sqrt( (1 - tanφ)/(1 + tanφ) ) dφ from -π/4 to π/4.

Simplifying the integrand: sqrt( (1 - tanφ)/(1 + tanφ) ). Let's rationalize this expression. Multiply numerator and denominator inside the square root by (1 - tanφ):

sqrt( (1 - tanφ)^2 / (1 - tan²φ) ). Wait, that's not helpful. Alternatively, note that (1 - tanφ)/(1 + tanφ) can be written as [cosφ - sinφ]/[cosφ + sinφ] by multiplying numerator and denominator by cosφ. Let's see:

(1 - tanφ)/(1 + tanφ) = (cosφ - sinφ)/(cosφ + sinφ). Let me check:

Multiply numerator and denominator by cosφ:

(1 - tanφ) * cosφ = cosφ - sinφ

(1 + tanφ) * cosφ = cosφ + sinφ

Yes, so (1 - tanφ)/(1 + tanφ) = (cosφ - sinφ)/(cosφ + sinφ). Then, sqrt of that is sqrt( (cosφ - sinφ)/(cosφ + sinφ) ). Let me write this as sqrt( (cosφ - sinφ)/(cosφ + sinφ) ). Maybe this can be simplified further. Let's note that (cosφ - sinφ)/(cosφ + sinφ) = [1 - tanφ]/[1 + tanφ], but perhaps another angle identity. Let's consider that cosφ - sinφ = sqrt(2) cos(φ + π/4), and cosφ + sinφ = sqrt(2) sin(φ + π/4). Let me verify:

cosφ - sinφ = sqrt(2) cos(φ + π/4). Because:

sqrt(2) cos(φ + π/4) = sqrt(2)[cosφ cos(π/4) - sinφ sin(π/4)] = sqrt(2)[ (cosφ)(sqrt(2)/2) - (sinφ)(sqrt(2)/2) ] = (sqrt(2)*sqrt(2)/2)(cosφ - sinφ) = (2/2)(cosφ - sinφ) = cosφ - sinφ. Yes.

Similarly, cosφ + sinφ = sqrt(2) sin(φ + π/4 + π/2) or perhaps another angle. Wait, let's check:

sqrt(2) sin(φ + π/4) = sqrt(2)[sinφ cos(π/4) + cosφ sin(π/4)] = sqrt(2)[ (sinφ)(sqrt(2)/2) + (cosφ)(sqrt(2)/2) ] = (sqrt(2)*sqrt(2)/2)(sinφ + cosφ) = (2/2)(sinφ + cosφ) = sinφ + cosφ. Yes. So cosφ + sinφ = sqrt(2) sin(φ + π/4).

Therefore, the ratio (cosφ - sinφ)/(cosφ + sinφ) = [sqrt(2) cos(φ + π/4)] / [sqrt(2) sin(φ + π/4)] = cot(φ + π/4). Therefore, sqrt( (cosφ - sinφ)/(cosφ + sinφ) ) = sqrt( cot(φ + π/4) ) = [cot(φ + π/4)]^{1/2} = [cos(φ + π/4)/sin(φ + π/4)]^{1/2} = cot^{1/2}(φ + π/4).

But integrating cot^{1/2}(φ + π/4) dφ might not be straightforward. Alternatively, perhaps make a substitution θ = φ + π/4. Let θ = φ + π/4, so when φ = -π/4, θ = 0; when φ = π/4, θ = π/2. Then dθ = dφ. The integral becomes:

∫_{0}^{π/2} cot^{1/2}(θ) dθ.

But ∫ cot^{1/2}θ dθ is ∫ sqrt(cotθ) dθ. Let me recall that cotθ = cosθ/sinθ, so sqrt(cotθ) = (cosθ/sinθ)^{1/2} = cos^{1/2}θ / sin^{1/2}θ. This might relate to the Beta function again. Let me consider substitution t = sinθ. Let t = sinθ, then dt = cosθ dθ. Then sqrt(cotθ) = sqrt( cosθ / sinθ ) = sqrt( (sqrt(1 - t²)) / t ). Hmm, not sure. Alternatively, express in terms of t = θ. Alternatively, use substitution u = tanθ. Let u = tanθ, then θ from 0 to π/2 corresponds to u from 0 to ∞. Then cotθ = 1/u. So sqrt(cotθ) = u^{-1/2}. Also, dθ = du/(1 + u²). So the integral becomes ∫₀^∞ u^{-1/2} / (1 + u²) du. That's ∫₀^∞ u^{-1/2} / (1 + u²) du. This is a standard integral. Let me recall that ∫₀^∞ x^{m-1} / (1 + x)^n dx = B(m, n - m) for n > m > 0. But here, the denominator is 1 + u², not 1 + u. Let me consider substitution v = u². Let v = u², so u = v^{1/2}, du = (1/2)v^{-1/2} dv. Then the integral becomes:

∫₀^∞ (v^{-1/4}) / (1 + v) * (1/2) v^{-1/2} dv = (1/2) ∫₀^∞ v^{-3/4} / (1 + v) dv.

This is similar to the Beta function integral. Recall that ∫₀^∞ x^{k-1}/(1 + x)^{k + m} dx = B(k, m). Wait, but here it's ∫₀^∞ v^{-3/4}/(1 + v) dv. Let me set x = v, so the integral is ∫₀^∞ x^{-3/4}/(1 + x) dx. This is known to be B(1/4, 3/4) because ∫₀^∞ x^{c -1}/(1 + x)^{c + d} dx = B(c, d). Wait, more accurately, the integral ∫₀^∞ x^{s -1}/(1 + x)^t dx = B(s, t - s) when t > s > 0. Here, s = 1 - 3/4 = 1/4? Wait, let me check. Let me recall that ∫₀^∞ x^{k -1}/(1 + x)^{k + m)} dx = B(k, m). So if we have ∫₀^∞ x^{k -1}/(1 + x)^{n} dx = B(k, n - k) when n > k > 0. In our case, the integral is ∫₀^∞ x^{-3/4}/(1 + x) dx. Let me write x^{-3/4} as x^{(1/4) -1}, so k = 1/4, and n = 1. Then n - k = 1 - 1/4 = 3/4. Therefore, the integral is B(1/4, 3/4). 

The Beta function B(1/4, 3/4) is equal to Γ(1/4)Γ(3/4)/Γ(1). Since Γ(1) = 1, and Γ(1/4)Γ(3/4) = π / sin(π/4) by the reflection formula Γ(z)Γ(1 - z) = π / sin(π z). So Γ(1/4)Γ(3/4) = π / sin(π/4) = π / (√2/2) ) = 2π/√2 = π√2. Therefore, B(1/4, 3/4) = π√2. 

But wait, let's verify that. The reflection formula says Γ(z)Γ(1 - z) = π / sin(π z). So for z = 1/4, Γ(1/4)Γ(3/4) = π / sin(π/4) = π / (√2/2) = 2π/√2 = π√2. Yes. So B(1/4, 3/4) = π√2. Therefore, the integral ∫₀^∞ x^{-3/4}/(1 + x) dx = π√2. But our integral was (1/2) times this, so (1/2) * π√2 = π/√2. 

So going back through the substitutions, the integral ∫_{-1}^{1} (u + 1)^{-1/2} (1 - u)^{1/2} / (u² + 1) du equals π/√2. Therefore, the original integral after substitution was 2 times the integral from 0 to 1, which became this integral, which evaluated to π/√2. Wait, let's retrace:

Original integral after substitution was 2 ∫₀¹ t^{-1/2} (1 - t)^{1/2} / (2t² - 2t + 1) dt. Then we did substitution u = 2(t - 0.5), leading to ∫_{-1}^{1} ... du, which after substitutions became ∫_{-1}^{1} (u + 1)^{-1/2} (1 - u)^{1/2} / (u² + 1) du. Then through substitution, we found that this integral equals π/√2. Therefore, the original integral is 2 * (π/√2) = π√2. Wait, no. Wait, let's check:

Wait, when we did the substitution t = (u + 1)/2, the integral became 2 * ∫_{-1}^{1} ... du, which after simplification became ∫_{-1}^{1} ... du = π/√2. Therefore, the original integral is 2 * (π/√2) = π√2. Wait, no. Wait, no. Let me retrace:

Original integral after substitution t = x/2 became 2 ∫₀¹ t^{-1/2} (1 - t)^{1/2} / (2t² - 2t + 1) dt. Then we did substitution u = 2(t - 0.5), leading to the integral ∫_{-1}^{1} ... du. Then through substitutions, we found that integral equals π/√2. Therefore, the original integral is 2 * (π/√2) = π√2. Wait, no. Wait, the substitution steps:

Original integral after substitution t = x/2 was 2 ∫₀¹ ... dt. Then after substitution u = 2(t - 0.5), the integral became 2 * [integral over u from -1 to 1 of ... du/2], because dt = du/2. Wait, no. Let me check again:

When we did the substitution u = 2(t - 0.5), then t = (u + 1)/2, dt = du/2. So the integral 2 ∫₀¹ ... dt becomes 2 ∫_{-1}^{1} ... (du/2) = ∫_{-1}^{1} ... du. Then after substitutions, that integral became π/√2. Therefore, the original integral is π/√2. Wait, but earlier steps suggested that after substitution, the integral became ∫_{-1}^{1} ... du which evaluated to π/√2. Therefore, the original integral is π/√2. But wait, let's check the steps again carefully.

Original integral: ∫₀² x^{-1/2} (2 - x)^{1/2} / [1 - 0.5x(2 - x)] dx.

Substitution t = x/2, x = 2t, dx = 2dt. Then integral becomes:

∫₀¹ (2t)^{-1/2} (2 - 2t)^{1/2} / [1 - 0.5*(2t)(2 - 2t)] * 2 dt

Simplify:

(2t)^{-1/2} = 2^{-1/2} t^{-1/2}

(2 - 2t)^{1/2} = 2^{1/2} (1 - t)^{1/2}

Denominator: 1 - 0.5*(2t)(2 - 2t) = 1 - 0.5*(4t - 4t²) = 1 - 2t + 2t²

So the integrand becomes:

[2^{-1/2} t^{-1/2} * 2^{1/2} (1 - t)^{1/2} ] / (2t² - 2t + 1) * 2 dt

The 2^{-1/2} and 2^{1/2} cancel, leaving:

[ t^{-1/2} (1 - t)^{1/2} / (2t² - 2t + 1) ] * 2 dt

So integral is 2 ∫₀¹ t^{-1/2} (1 - t)^{1/2} / (2t² - 2t + 1) dt

Then substitution u = 2(t - 0.5), t = (u + 1)/2, dt = du/2. Limits u from -1 to 1.

Integral becomes:

2 ∫_{-1}^{1} [ ((u + 1)/2)^{-1/2} (1 - (u + 1)/2)^{1/2} / (2*((u + 1)/2)^2 - 2*((u + 1)/2) + 1) ] * (du/2)

Simplify each part:

((u + 1)/2)^{-1/2} = 2^{1/2} (u + 1)^{-1/2}

(1 - (u + 1)/2)^{1/2} = ( (2 - u - 1)/2 )^{1/2} = ( (1 - u)/2 )^{1/2} = 2^{-1/2} (1 - u)^{1/2}

Denominator: 2*((u + 1)/2)^2 - 2*((u + 1)/2) + 1

= 2*( (u + 1)^2 /4 ) - (u + 1) + 1

= ( (u + 1)^2 )/2 - u -1 +1

= (u² + 2u + 1)/2 - u

= (u² + 2u + 1 - 2u)/2

= (u² + 1)/2

So denominator is (u² + 1)/2

Putting it all together:

2 * [ 2^{1/2} (u + 1)^{-1/2} * 2^{-1/2} (1 - u)^{1/2} / ( (u² + 1)/2 ) ] * (du/2)

Simplify constants:

2^{1/2} * 2^{-1/2} = 1

Denominator (u² + 1)/2 becomes multiplying by 2/(u² + 1)

Then multiplied by du/2:

So overall:

2 * [ (u + 1)^{-1/2} (1 - u)^{1/2} * 2/(u² + 1) ] * (du/2)

The 2 and the 1/2 cancel, leaving:

∫_{-1}^{1} (u + 1)^{-1/2} (1 - u)^{1/2} / (u² + 1) du

Then, through substitution, we found this integral equals π/√2. Therefore, the original integral is π/√2. 

But wait, in the steps above, after substitution, the integral became ∫_{-1}^{1} ... du = π/√2. Therefore, the original integral is π/√2. 

But let's verify this with numerical approximation. Let's compute π/√2 numerically. π is approximately 3.1415926536, √2 is approximately 1.4142135624. So π/√2 ≈ 3.1415926536 / 1.4142135624 ≈ 2.2214414691. Let's check this with a numerical approximation of the original integral.

Alternatively, perhaps I made a mistake in the substitution steps. Let me verify with a numerical integral. Let's compute the original integral numerically. The original integral is ∫₀² x^{-1/2} (2 - x)^{1/2} / [1 - 0.5x(2 - x)] dx. Let's approximate this using a calculator or software. However, since I can't compute it here, I'll proceed with the analytical result.

But according to the steps, the integral evaluates to π/√2. Therefore, the exact answer is π/√2, and the numerical approximation is approximately 2.2214414691. Rounded to 10 decimal places, that's 2.2214414691.

But let me check the steps again to ensure no mistakes. The key step was transforming the integral into a form that relates to the Beta function, and through substitutions, we arrived at an integral that evaluates to π/√2. Therefore, the final answer should be π/√2.
</think>

{"answer": "\\frac{\\pi}{\\sqrt{2}}", "numerical_answer": "2.2214414691"}