Let's address the integral step-by-step:

\[
I = \int_{1}^{\infty} x (x^2 - 1)^{2 - \frac{3}{2}} e^{-0.5^2 x^2} H_{4}(0.5x)\,dx
\]

Let's break it down:

1. **Simplify the exponent**: \(2 - \frac{3}{2} = \frac{1}{2}\)
2. **So, the integral is:**

\[
I = \int_{1}^{\infty} x (x^2 - 1)^{1/2} e^{-0.25 x^2} H_{4}(0.5x)\, dx
\]

The terms:
- \(H_4(x)\) is the 4th Hermite polynomial
- The substitution \(H_{2 \times 2} (0.5x) = H_4(0.5x)\).

Recall the form of the 4th Hermite polynomial:

\[
H_4(x) = 16x^4 - 48x^2 + 12
\]
So:
\[
H_4(0.5x) = 16 (0.5x)^4 - 48 (0.5x)^2 + 12 = 1x^4 - 12x^2 + 12
\]

Full expansion:
- \((0.5x)^4 = 0.0625x^4\), \(16 \times 0.0625 = 1x^4\)
- \((0.5x)^2 = 0.25x^2\), \(-48 \times 0.25 = -12x^2\)
- The constant is \(+12\)

So:
\[
H_4(0.5x) = x^4 - 12x^2 + 12
\]

Therefore, the integral becomes:
\[
I = \int_{1}^{\infty} x (x^2 - 1)^{1/2} e^{-0.25 x^2} (x^4 - 12x^2 + 12)\, dx
\]

Let's split:
\[
I = \int_{1}^{\infty} x (x^2 - 1)^{1/2} e^{-0.25 x^2} x^4\, dx
- 12\int_{1}^{\infty} x (x^2 - 1)^{1/2} e^{-0.25 x^2} x^2\, dx
+ 12\int_{1}^{\infty} x (x^2 - 1)^{1/2} e^{-0.25 x^2} dx
\]

Now, let's use the substitution \(u = x^2\), \(du = 2x dx \Rightarrow x dx = \frac{1}{2} du\), when \(x=1\), \(u=1\), as \(x \to \infty, u \to \infty\):

Let’s substitute:

- \(x (x^2-1)^{1/2} = (x^2-1)^{1/2} x\)
- \(x^4 = (x^2)^2 = u^2\)
- \(x^2 = u\)
- \(x dx = \frac{1}{2} du\)
- \(x^2-1 = u-1\)
- \(e^{-0.25 x^2} = e^{-0.25 u}\)

Let’s convert each term:

**First term:**
\[
\int_{1}^{\infty} x (x^2-1)^{1/2} e^{-0.25x^2} x^4 dx = \int_{u=1}^{\infty} (u-1)^{1/2} e^{-0.25 u} u^2 \cdot \frac{1}{2} du
\]

**Second term:**
\[
-12 \int_{1}^{\infty} x (x^2-1)^{1/2} e^{-0.25x^2} x^2 dx = -12 \int_{u=1}^{\infty} (u-1)^{1/2} e^{-0.25 u} u \cdot \frac{1}{2} du
\]

**Third term:**
\[
+12 \int_{1}^{\infty} x (x^2-1)^{1/2} e^{-0.25x^2} dx = +12 \int_{u=1}^{\infty} (u-1)^{1/2} e^{-0.25 u} \frac{1}{2} du
\]

So, bring together:
\[
I = \frac{1}{2}\int_{1}^{\infty} (u-1)^{1/2} e^{-0.25u} (u^2 - 12u + 12) du
\]

Or, more simply:

\[
I = \frac{1}{2} \int_{1}^{\infty} (u-1)^{1/2} e^{-0.25u} (u^2 - 12u + 12)\, du
\]

Now, let's substitute \(t = u-1\), so \(u = t + 1\), \(du = dt\), \(u = 1 \implies t = 0\), \(u = \infty \implies t = \infty\):

So,
- \((u-1)^{1/2} = t^{1/2}\)
- \(e^{-0.25u} = e^{-0.25 t} e^{-0.25}\)
- \((u^2 - 12u + 12) = (t+1)^2 - 12(t+1) + 12 = t^2 + 2t + 1 - 12t - 12 + 12 = t^2 - 10t + 1\)

So:

\[
I = \frac{1}{2} \int_{t=0}^{\infty} t^{1/2} e^{-0.25 t} e^{-0.25} [ t^2 - 10 t + 1 ] dt
\]

Factor out \(e^{-0.25}\):

\[
I = \frac{e^{-0.25}}{2} \int_{0}^{\infty} t^{1/2} e^{-0.25 t} (t^2 - 10t + 1) dt
\]

Now write as sum:

\[
I = \frac{e^{-0.25}}{2} \left[
\int_{0}^{\infty} t^{5/2} e^{-0.25 t} dt
-10 \int_{0}^{\infty} t^{3/2} e^{-0.25 t} dt
+\int_{0}^{\infty} t^{1/2} e^{-0.25 t} dt
\right]
\]

The integrals are of the form:

\[
\int_0^\infty t^{\alpha} e^{-\beta t} dt = \frac{\Gamma(\alpha+1)}{\beta^{\alpha+1}}
\]

Here, \(\beta = 0.25\), and the powers are \(5/2, 3/2, 1/2\):

- \(\Gamma\left(\frac{7}{2}\right), \Gamma\left(\frac{5}{2}\right), \Gamma\left(\frac{3}{2}\right)\)
- \(\beta^{\alpha+1}\): for \(5/2\): \(0.25^{7/2} = (1/4)^{7/2} = 1 / 2^{7} = 1/128\)
- for \(3/2\): \(0.25^{5/2} = (1/4)^{5/2} = 1/32\)
- for \(1/2\): \(0.25^{3/2} = (1/4)^{3/2} = 1/8\)

So:

\[
I = \frac{e^{-0.25}}{2}
\left[
\frac{\Gamma(7/2)}{1/128}
-10 \frac{\Gamma(5/2)}{1/32}
+\frac{\Gamma(3/2)}{1/8}
\right]
\]
i.e.
\[
I = \frac{e^{-0.25}}{2}
\left[
128 \Gamma(7/2)
-320 \Gamma(5/2)
+8\Gamma(3/2)
\right]
\]

Let's recall the values for the Gamma function at half-integers:

- \(\Gamma(n+1/2) = \frac{(2n)!}{4^n n!} \sqrt{\pi}\)
But more practically:
- \(\Gamma(\frac{3}{2}) = \frac{1}{2} \sqrt{\pi}\)
- \(\Gamma(\frac{5}{2}) = \frac{3}{4} \sqrt{\pi}\)
- \(\Gamma(\frac{7}{2}) = \frac{15}{8} \sqrt{\pi}\)

So:

- \(128 \Gamma(7/2) = 128 \cdot \frac{15}{8} \sqrt{\pi} = 16 \times 15 \sqrt{\pi} = 240 \sqrt{\pi}\)
- \(320 \Gamma(5/2) = 320 \cdot \frac{3}{4} \sqrt{\pi} = 80 \times 3 \sqrt{\pi} = 240 \sqrt{\pi}\)
- \(8 \Gamma(3/2) = 8 \times \frac{1}{2} \sqrt{\pi} = 4 \sqrt{\pi}\)

So: \(240\sqrt{\pi} - 240\sqrt{\pi} + 4\sqrt{\pi} = 4 \sqrt{\pi}\)

Thus,

\[
I = \frac{e^{-0.25}}{2} \times 4\sqrt{\pi} = 2 e^{-0.25} \sqrt{\pi}
\]

---

**So, the exact answer is:**
\[
I = 2 e^{-0.25}\sqrt{\pi}
\]

---

### Evaluate numerically

- \(e^{-0.25} \approx 0.7788007831\)
- \(\sqrt{\pi} \approx 1.7724538509\)
- \(2 \times 0.7788007831 \times 1.7724538509 \approx 2.7578609806\)

---

### Final JSON answer

```json
{"answer": "2 e^{-0.25} \\sqrt{\\pi}", "numerical_answer": "2.7578609806"}
```