Let's denote the given integral as
\[
I = \int_0^1 \frac{x^{2023} - x^{23}}{\ln x} \, dx.
\]

### Step 1: Analytic Computation

Recall a useful integral identity:
\[
\int_0^1 \frac{x^a - x^b}{\ln x}\,dx = \ln\left(\frac{a+1}{b+1}\right),
\]
for \(a, b > -1\). This comes from the result:
\[
\int_0^1 \frac{x^k}{\ln x}\,dx = \frac{1}{k+1}, \text{ (via Laplace transform or by integrating by parts) }
\]
But more precisely, the identity is:
\[
\int_0^1 \frac{x^a - x^b}{\ln x}\,dx = \ln\left(\frac{b+1}{a+1}\right)
\]

But let's verify carefully:

Let’s recall for \(c > -1\),
\[
I(c) = \int_0^1 \frac{x^c}{\ln x} dx = \int_0^1 \int_0^c x^t\,dt\, dx \text{ (by Fubini / integral representation) }
\]
But more straightforward is to recall:
Let’s consider the Laplace transform representation:
\[
\frac{1}{\ln x} = \int_0^\infty e^{-t \ln x} dt = \int_0^\infty x^{-t}dt
\]
But perhaps simpler: Let's recall:

It's well-known that:
\[
\int_0^1 x^{k} dx = \frac{1}{k+1}
\]
and
\[
\int_0^1 \frac{x^a - x^b}{\ln x} dx = \ln\left(\frac{b+1}{a+1}\right)
\]
(This is correct; we can see e.g. [source](https://math.stackexchange.com/questions/53009/evaluate-int-01-fracx^a-x^b-ln-x-dx-without-lhopital) )

Thus, applying this to \(a = 2023\), \(b = 23\):

\[
I = \int_0^1 \frac{x^{2023} - x^{23}}{\ln x} dx = \ln\left(\frac{23+1}{2023+1}\right) = \ln\left(\frac{24}{2024}\right) = \ln\left(\frac{1}{84.3333\dots}\right)
\]

Alternatively,
\[
\ln\left(\frac{24}{2024}\right) = \ln(24) - \ln(2024)
\]

### Step 2: Numerical Approximation

Now calculate:

- \(\ln 24 \approx 3.1780538303479458\)
- \(\ln 2024 \approx 7.616146558451492\)

Therefore,

\[
\ln(24) - \ln(2024) \approx 3.17805383035 - 7.61614655845 = -4.43809272810
\]

Rounded to 10 decimal places: \(-4.4380927281\)

### Final Answer

```json
{"answer": "\\ln\\left(\\frac{24}{2024}\\right)", "numerical_answer": "-4.4380927281"}
```