# Evaluating $\int\limits_{0}^{2.0}x\cos\left(1.0\sqrt{x(2.0-x)}\right)dx$

## Step 1: Let's examine the structure of this integral
I'll note that the integral has a symmetric structure around $x = 1$. Let's make a substitution to exploit this symmetry.

Let's observe that $x(2-x) = 2x - x^2 = -(x^2 - 2x + 1) + 1 = -(x-1)^2 + 1$

This means $\sqrt{x(2-x)} = \sqrt{-(x-1)^2 + 1} = \sqrt{1-(x-1)^2}$

## Step 2: Symmetry consideration
Consider the substitution $u = 2-x$. When $x = 0$, $u = 2$, and when $x = 2$, $u = 0$.

Under this substitution:
$dx = -du$
$\sqrt{x(2-x)} = \sqrt{u(2-u)}$

So the integral becomes:
$\int\limits_{0}^{2.0}x\cos\left(1.0\sqrt{x(2.0-x)}\right)dx = \int\limits_{2}^{0}(2-u)\cos\left(1.0\sqrt{u(2.0-u)}\right)(-du)$
$= \int\limits_{0}^{2.0}(2-u)\cos\left(1.0\sqrt{u(2.0-u)}\right)du$

Adding the original integral and this transformed version:
$\int\limits_{0}^{2.0}x\cos\left(1.0\sqrt{x(2.0-x)}\right)dx + \int\limits_{0}^{2.0}(2-x)\cos\left(1.0\sqrt{x(2.0-x)}\right)dx$
$= \int\limits_{0}^{2.0}2\cos\left(1.0\sqrt{x(2.0-x)}\right)dx$
$= 2\int\limits_{0}^{2.0}\cos\left(1.0\sqrt{x(2.0-x)}\right)dx$

Therefore:
$\int\limits_{0}^{2.0}x\cos\left(1.0\sqrt{x(2.0-x)}\right)dx = \int\limits_{0}^{2.0}\cos\left(1.0\sqrt{x(2.0-x)}\right)dx$

## Step 3: Solving the simplified integral
Let's make another substitution. Let $t = x-1$, so $x = t+1$ and $dx = dt$.
When $x = 0$, $t = -1$, and when $x = 2$, $t = 1$.

With this substitution:
$\sqrt{x(2-x)} = \sqrt{(t+1)(2-(t+1))} = \sqrt{(t+1)(1-t)} = \sqrt{1-t^2}$

So our integral becomes:
$\int\limits_{0}^{2.0}\cos\left(1.0\sqrt{x(2.0-x)}\right)dx = \int\limits_{-1}^{1}\cos\left(1.0\sqrt{1-t^2}\right)dt$

Now let's use the substitution $t = \sin\theta$, which gives $dt = \cos\theta\,d\theta$.
When $t = -1$, $\theta = -\pi/2$, and when $t = 1$, $\theta = \pi/2$.

With this:
$\sqrt{1-t^2} = \sqrt{1-\sin^2\theta} = \sqrt{\cos^2\theta} = |\cos\theta| = \cos\theta$ (since $\theta \in [-\pi/2, \pi/2]$)

So our integral becomes:
$\int\limits_{-\pi/2}^{\pi/2}\cos(1.0\cos\theta)\cos\theta\,d\theta$

## Step 4: Evaluate using properties of even/odd functions
Note that $\cos(1.0\cos\theta)$ is an even function of $\theta$, and $\cos\theta$ is also even.
So the integrand $\cos(1.0\cos\theta)\cos\theta$ is even.

For an even function integrated over $[-\pi/2, \pi/2]$, we have:
$\int\limits_{-\pi/2}^{\pi/2}\cos(1.0\cos\theta)\cos\theta\,d\theta = 2\int\limits_{0}^{\pi/2}\cos(1.0\cos\theta)\cos\theta\,d\theta$

## Step 5: Use properties of Bessel functions
The integral $\int\limits_{0}^{\pi/2}\cos(z\cos\theta)\cos\theta\,d\theta$ equals $\frac{\pi}{2}J_1(z)$, where $J_1$ is the Bessel function of the first kind of order 1.

With $z = 1.0$, we have:
$\int\limits_{0}^{2.0}x\cos\left(1.0\sqrt{x(2.0-x)}\right)dx = \pi J_1(1.0)$

## Step 6: Calculate the numerical value
The value of $J_1(1.0) \approx 0.4400505857$

Therefore:
$\int\limits_{0}^{2.0}x\cos\left(1.0\sqrt{x(2.0-x)}\right)dx = \pi J_1(1.0) \approx \pi \cdot 0.4400505857 \approx 1.3823562678$

{"answer": "\pi J_1(1.0)", "numerical_answer": "1.3823562678"}