We wish to evaluate

  I = ∫₁^(∞) x (x² – 1²)^(2 – 3/2) e^(–0.5² x²) H₍₂*2₎(0.5x) dx.

Step 1. Write the integral in a simpler form.

Notice that:
• 2 – 3/2 = 1/2, so the power is ½.
• 0.5² = 0.25.
• H₍₂*2₎(0.5x) means the Hermite polynomial of order 4 evaluated at 0.5x.

Recall that the Hermite polynomial H₄(u) is given by:
  H₄(u) = 16u⁴ – 48u² + 12.
Thus, with u = 0.5x we have:
  H₄(0.5x) = 16(0.5x)⁴ – 48(0.5x)² + 12
        = 16(x⁴ / 16) – 48(x²/4) + 12
        = x⁴ – 12x² + 12.

Thus the integral becomes

  I = ∫₁^(∞) x (x² – 1)^(1/2) e^(–x²/4) (x⁴ – 12x² + 12) dx.

Step 2. Make a substitution to simplify further.

Let u = x² – 1 so that
  du/dx = 2x  ⟹  x dx = du/2.
When x = 1, u = 0; as x → ∞, u → ∞.

Also, note that x² = u + 1 and hence
  x⁴ = (u + 1)².
The polynomial becomes:
  x⁴ – 12x² + 12 = (u + 1)² – 12(u + 1) + 12.
Expanding:
  (u + 1)² = u² + 2u + 1,
so
  x⁴ – 12x² + 12 = u² + 2u + 1 – 12u – 12 + 12 = u² – 10u + 1.

Also, the factor x (x² – 1)^(1/2) dx becomes:
  x (√(x²–1)) dx = √u · dx · x = (du/(2)) √u.

Thus the integral becomes

  I = 1/2 ∫₀^(∞) (u² – 10u + 1) u^(1/2) e^(–(u+1)/4) du
     = e^(–1/4)/2 ∫₀^(∞) (u² – 10u + 1) u^(1/2) e^(–u/4) du.

Step 3. Express the integral as a sum of Gamma integrals.

Write the integrand as
  (u² – 10u + 1) u^(1/2) = u^(5/2) – 10 u^(3/2) + u^(1/2).

Thus

  I = (e^(–1/4)/2)[∫₀^(∞) u^(5/2) e^(–u/4) du – 10∫₀^(∞) u^(3/2)e^(–u/4)du + ∫₀^(∞) u^(1/2)e^(–u/4)du].

Recall that
  ∫₀^(∞) u^(α) e^(–u/4) du = Γ(α+1) · 4^(α+1).

Thus, term‐by‐term:
1. For u^(5/2): α = 5/2,
  ∫ = Γ(7/2) · 4^(7/2).
2. For u^(3/2): α = 3/2,
  ∫ = Γ(5/2) · 4^(5/2).
3. For u^(1/2): α = 1/2,
  ∫ = Γ(3/2) · 4^(3/2).

Our expression becomes

  I = (e^(–1/4)/2)[Γ(7/2) 4^(7/2) – 10 Γ(5/2) 4^(5/2) + Γ(3/2) 4^(3/2)].

Step 4. Substitute the Gamma function values and simplify.

We have:
  Γ(3/2) = (√π)/2,
  Γ(5/2) = (3√π)/4,
  Γ(7/2) = (15√π)/8.

Also, note that:
  4^(3/2) = 8,
  4^(5/2) = 32,
  4^(7/2) = 128.

Substitute these:
  I = (e^(–1/4)/2)[ (15√π/8)*128 – 10*(3√π/4)*32 + (√π/2)*8 ].

Now simplify each term:
• First term: (15√π/8)*128 = 15√π · 16 = 240√π.
• Second term: 10*(3√π/4)*32 = 10 · 3√π · 8 = 240√π.
• Third term: (√π/2)*8 = 4√π.

Thus, inside the bracket we have:
  240√π – 240√π + 4√π = 4√π.

So,
  I = (e^(–1/4)/2)[4√π] = 2√π e^(–1/4).

Step 5. Provide the numerical approximation.

We have:
  √π ≈ 1.7724538509,
  e^(–1/4) = e^(–0.25) ≈ 0.7788007831.
Thus,
  I ≈ 2 × 1.7724538509 × 0.7788007831 ≈ 3.5449077018 × 0.7788007831 ≈ 2.7621802552.

Step 6. Present the final answer in the required JSON format.

{"answer": "2\\sqrt{\\pi}e^{-\\frac{1}{4}}", "numerical_answer": "2.7621802552"}