


To solve the definite integral \(\int_{0}^{2} x \arctan\left(\sqrt{x(2-x)}\right) \, dx\), we proceed as follows:

### Step 1: Simplify the Integrand
First, note that \(x(2-x) = 2x - x^2 = 1 - (x-1)^2\) (by completing the square). Let \(t = x - 1\), so \(x = t + 1\) and \(dx = dt\). The limits of integration change from \(x=0\) to \(t=-1\) and \(x=2\) to \(t=1\). The integral becomes:
\[
\int_{-1}^{1} (t + 1) \arctan\left(\sqrt{1 - t^2}\right) \, dt
\]

### Step 2: Split the Integral
Split the integral into two parts:
\[
\int_{-1}^{1} t \arctan\left(\sqrt{1 - t^2}\right) \, dt + \int_{-1}^{1} \arctan\left(\sqrt{1 - t^2}\right) \, dt
\]

### Step 3: Evaluate the First Integral
The first integrand \(t \arctan\left(\sqrt{1 - t^2}\right)\) is an odd function (since \(f(-t) = -f(t)\)). Over the symmetric interval \([-1, 1]\), the integral of an odd function is zero:
\[
\int_{-1}^{1} t \arctan\left(\sqrt{1 - t^2}\right) \, dt = 0
\]

### Step 4: Evaluate the Second Integral
The second integrand \(\arctan\left(\sqrt{1 - t^2}\right)\) is even (since \(f(-t) = f(t)\)). Thus:
\[
\int_{-1}^{1} \arctan\left(\sqrt{1 - t^2}\right) \, dt = 2 \int_{0}^{1} \arctan\left(\sqrt{1 - t^2}\right) \, dt
\]

### Step 5: Substitute \(t = \sin\theta\)
Let \(t = \sin\theta\), so \(dt = \cos\theta \, d\theta\) and \(\sqrt{1 - t^2} = \cos\theta\). The limits change from \(t=0\) to \(\theta=0\) and \(t=1\) to \(\theta=\pi/2\). The integral becomes:
\[
2 \int_{0}^{\pi/2} \arctan(\cos\theta) \cdot \cos\theta \, d\theta
\]

### Step 6: Integration by Parts
Let \(u = \arctan(\cos\theta)\) and \(dv = \cos\theta \, d\theta\). Then \(du = \frac{-\sin\theta}{1 + \cos^2\theta} \, d\theta\) and \(v = \sin\theta\). Integration by parts gives:
\[
\left. u v \right|_{0}^{\pi/2} - \int_{0}^{\pi/2} v \, du
\]
The boundary term \(\left. u v \right|_{0}^{\pi/2}\) is zero (since \(\arctan(0) \cdot 1 = 0\) and \(\arctan(1) \cdot 0 = 0\)). The remaining integral simplifies to:
\[
\int_{0}^{\pi/2} \frac{\sin^2\theta}{1 + \cos^2\theta} \, d\theta
\]

### Step 7: Simplify the Integrand
Using \(\sin^2\theta = 1 - \cos^2\theta\), rewrite the integrand:
\[
\frac{1 - \cos^2\theta}{1 + \cos^2\theta} = \frac{2}{1 + \cos^2\theta} - 1
\]
Thus, the integral becomes:
\[
2 \int_{0}^{\pi/2} \frac{1}{1 + \cos^2\theta} \, d\theta - \int_{0}^{\pi/2} 1 \, d\theta
\]

### Step 8: Evaluate the Integrals
The first integral \(\int_{0}^{\pi/2} \frac{1}{1 + \cos^2\theta} \, d\theta\) uses the substitution \(t = \tan\theta\), leading to \(\frac{\pi}{2\sqrt{2}}\). The second integral is \(\frac{\pi}{2}\). Combining these:
\[
2 \cdot \frac{\pi}{2\sqrt{2}} - \frac{\pi}{2} = \frac{\pi}{\sqrt{2}} - \frac{\pi}{2}
\]

### Final Result
The exact value of the integral is \(\frac{\pi}{\sqrt{2}} - \frac{\pi}{2}\).

### Numerical Approximation
Using \(\pi \approx 3.141592653589793\) and \(\sqrt{2} \approx 1.4142135623730951\), the numerical approximation is approximately \(0.6506451423\) (rounded to 10 decimal places).

{"answer": "\\frac{\\pi}{\\sqrt{2}} - \\frac{\\pi}{2}", "numerical_answer": "0.6506451423"}