To solve the definite integral \(\int_{-4}^4 e^{|x|} \cdot \{x\} \, dx\), where \(\{x\}\) denotes the fractional part of \(x\), we follow these steps:

### Step 1: Understand the Fractional Part Function
The fractional part of \(x\) is defined as \(\{x\} = x - \lfloor x \rfloor\), where \(\lfloor x \rfloor\) is the floor function. For any real number \(x\), \(0 \leq \{x\} < 1\).

### Step 2: Split the Integral Based on the Floor Function
The interval \([-4, 4]\) can be split into subintervals where the floor function \(\lfloor x \rfloor\) is constant. These subintervals are:
- \([-4, -3)\), \(\lfloor x \rfloor = -4\), \(\{x\} = x + 4\)
- \([-3, -2)\), \(\lfloor x \rfloor = -3\), \(\{x\} = x + 3\)
- \([-2, -1)\), \(\lfloor x \rfloor = -2\), \(\{x\} = x + 2\)
- \([-1, 0)\), \(\lfloor x \rfloor = -1\), \(\{x\} = x + 1\)
- \([0, 1)\), \(\lfloor x \rfloor = 0\), \(\{x\} = x\)
- \([1, 2)\), \(\lfloor x \rfloor = 1\), \(\{x\} = x - 1\)
- \([2, 3)\), \(\lfloor x \rfloor = 2\), \(\{x\} = x - 2\)
- \([3, 4)\), \(\lfloor x \rfloor = 3\), \(\{x\} = x - 3\)
- At \(x = 4\), \(\{4\} = 0\)

### Step 3: Compute the Integral Over Each Subinterval
Since \(e^{|x|}\) is symmetric and \(\{x\}\) changes definition at integer points, we compute the integral piecewise:

\[
\int_{-4}^4 e^{|x|} \cdot \{x\} \, dx = \sum_{k=-4}^3 \int_{k}^{k+1} e^{|x|} \cdot (x - k) \, dx
\]

However, due to the absolute value \(|x|\), we split the integral into negative and positive regions:

#### For \(x \in [-4, 0]\):
\[
\int_{-4}^0 e^{|x|} \cdot \{x\} \, dx = \int_{-4}^{-3} e^{-x} (x + 4) \, dx + \int_{-3}^{-2} e^{-x} (x + 3) \, dx + \int_{-2}^{-1} e^{-x} (x + 2) \, dx + \int_{-1}^{0} e^{-x} (x + 1) \, dx
\]

#### For \(x \in [0, 4]\):
\[
\int_{0}^4 e^{|x|} \cdot \{x\} \, dx = \int_{0}^{1} e^{x} x \, dx + \int_{1}^{2} e^{x} (x - 1) \, dx + \int_{2}^{3} e^{x} (x - 2) \, dx + \int_{3}^{4} e^{x} (x - 3) \, dx
\]

### Step 4: Compute Each Integral
We compute each integral separately using integration by parts where necessary.

#### Negative Region:
1. \(\int_{-4}^{-3} e^{-x} (x + 4) \, dx\):
   Let \(u = x + 4\), \(dv = e^{-x} dx\):
   \[
   = \left[ -e^{-x} (x + 4) \right]_{-4}^{-3} + \int_{-4}^{-3} e^{-x} dx = -e^{3} (-3 + 4) + e^{4} (-4 + 4) + \left[ -e^{-x} \right]_{-4}^{-3} = -e^{3} + 0 + (-e^{3} + e^{4}) = e^{4} - 2e^{3}
   \]

2. \(\int_{-3}^{-2} e^{-x} (x + 3) \, dx\):
   Similarly:
   \[
   = e^{3} - 2e^{2}
   \]

3. \(\int_{-2}^{-1} e^{-x} (x + 2) \, dx\):
   \[
   = e^{2} - 2e^{1}
   \]

4. \(\int_{-1}^{0} e^{-x} (x + 1) \, dx\):
   \[
   = e^{1} - 2e^{0}
   \]

Summing these:
\[
\text{Negative region} = (e^{4} - 2e^{3}) + (e^{3} - 2e^{2}) + (e^{2} - 2e^{1}) + (e^{1} - 2) = e^{4} - e^{3} - e^{2} - e^{1} - 2
\]

#### Positive Region:
1. \(\int_{0}^{1} e^{x} x \, dx\):
   Using integration by parts:
   \[
   = \left[ e^{x} x \right]_0^1 - \int_0^1 e^{x} dx = e^{1} - (e^{1} - 1) = 1
   \]

2. \(\int_{1}^{2} e^{x} (x - 1) \, dx\):
   Let \(u = x - 1\), \(dv = e^{x} dx\):
   \[
   = \left[ e^{x} (x - 1) \right]_1^2 - \int_1^2 e^{x} dx = e^{2} - 0 - (e^{2} - e^{1}) = e^{1}
   \]

3. \(\int_{2}^{3} e^{x} (x - 2) \, dx\):
   Similarly:
   \[
   = e^{2}
   \]

4. \(\int_{3}^{4} e^{x} (x - 3) \, dx\):
   \[
   = e^{3}
   \]

Summing these:
\[
\text{Positive region} = 1 + e^{1} + e^{2} + e^{3}
\]

### Step 5: Combine Results
Adding the negative and positive regions:
\[
\int_{-4}^4 e^{|x|} \cdot \{x\} \, dx = (e^{4} - e^{3} - e^{2} - e^{1} - 2) + (1 + e^{1} + e^{2} + e^{3}) = e^{4} - 1
\]

### Step 6: Numerical Approximation
Compute \(e^{4} - 1\):
\[
e^{4} \approx 54.5981500331 \\
e^{4} - 1 \approx 53.5981500331
\]

### Final Answer
```json
{"answer": "e^{4} - 1", "numerical_answer": "53.5981500331"}
```