

To solve the definite integral \(\int_{0}^{2}\frac{x^{-1/2}(2-x)^{-1/2}}{\sqrt{1+x(2-x)}}T_{3}\left(\sqrt{1+x(2-x)}\right)dx\), we proceed as follows:

### Step 1: Simplify the integrand using Chebyshev polynomials
The Chebyshev polynomial of the first kind \(T_3(z)\) is given by \(T_3(z) = 4z^3 - 3z\). Let \(u = \sqrt{1 + x(2 - x)}\), so \(T_3(u) = 4u^3 - 3u\). Substituting this into the integrand:
\[
\frac{x^{-1/2}(2-x)^{-1/2}}{u} \cdot (4u^3 - 3u) = x^{-1/2}(2-x)^{-1/2} \cdot (4u^2 - 3).
\]
Since \(u^2 = 1 + x(2 - x)\), we have \(4u^2 - 3 = 4(1 + x(2 - x)) - 3 = 1 + 4x(2 - x)\). Thus, the integrand simplifies to:
\[
x^{-1/2}(2-x)^{-1/2} \cdot \left(1 + 4x(2 - x)\right).
\]

### Step 2: Split the integral into two parts
The integral becomes:
\[
\int_{0}^{2} \frac{1}{\sqrt{x(2 - x)}} dx + 4 \int_{0}^{2} \sqrt{x(2 - x)} dx.
\]

### Step 3: Evaluate the first integral
The first integral is \(\int_{0}^{2} \frac{1}{\sqrt{x(2 - x)}} dx\). Using the substitution \(x = 2\sin^2\theta\) (with \(dx = 4\sin\theta\cos\theta d\theta\) and \(\sqrt{x(2 - x)} = 2\sin\theta\cos\theta\)), the integral transforms to:
\[
\int_{0}^{\pi/2} \frac{1}{2\sin\theta\cos\theta} \cdot 4\sin\theta\cos\theta d\theta = \int_{0}^{\pi/2} 2 d\theta = 2 \cdot \frac{\pi}{2} = \pi.
\]

### Step 4: Evaluate the second integral
The second integral is \(4 \int_{0}^{2} \sqrt{x(2 - x)} dx\). Note that \(x(2 - x) = 1 - (x - 1)^2\), so \(\sqrt{x(2 - x)}\) describes a semicircle of radius 1 centered at \(x = 1\). The integral of this semicircle over \([0, 2]\) is the area of the semicircle:
\[
\int_{0}^{2} \sqrt{x(2 - x)} dx = \frac{\pi \cdot 1^2}{2} = \frac{\pi}{2}.
\]
Thus, the second integral is \(4 \cdot \frac{\pi}{2} = 2\pi\).

### Step 5: Combine the results
Adding the two integrals gives:
\[
\pi + 2\pi = 3\pi.
\]

### Numerical Approximation
The numerical value of \(3\pi\) is approximately \(9.4247779608\) (rounded to 10 decimal places).

{"answer": "3\\pi", "numerical_answer": "9.4247779608"}