Let's compute the definite integral:
\[
I = \int_{0}^{7} \left( \sqrt[3]{\sqrt{x^2+1}+x} - \sqrt[3]{\sqrt{x^2+1}-x} \right) dx
\]

**Step 1: Simplify the integrand**

Let us set:
\[
f(x) = \sqrt[3]{\sqrt{x^2+1}+x} - \sqrt[3]{\sqrt{x^2+1}-x}
\]

Let \( y = \sqrt[3]{\sqrt{x^2+1}+x} \), \( z = \sqrt[3]{\sqrt{x^2+1}-x} \).

We aim to find an expression for \( f(x) \) that is more tractable.

Let’s consider a substitution.

Let’s set:
\[
t = \sqrt{x^2 + 1}
\]
Then \( x = \sqrt{t^2 - 1} \), and \( dx = \frac{t}{\sqrt{t^2-1}} dt \).

Also note \( t \) runs from \( x=0 \) (\(t=1\)) to \( x=7 \) (\(t=\sqrt{49+1}= \sqrt{50}=5\sqrt{2}\)).

Let’s see how the integrand transforms under this substitution:

\[
\sqrt[3]{t + \sqrt{t^2-1}} - \sqrt[3]{t - \sqrt{t^2-1}}
\]

Let’s let:
\[
a = t + \sqrt{t^2-1},\qquad b = t - \sqrt{t^2-1}
\]
Then \( a \cdot b = t^2 - (t^2-1) = 1 \implies b = 1/a \).

Then:
\[
\sqrt[3]{a} - \sqrt[3]{b} = \sqrt[3]{a} - \sqrt[3]{1/a} = \sqrt[3]{a} - \frac{1}{\sqrt[3]{a}} = y - \frac{1}{y}
\]

Let’s now express \( x \) in terms of \( y \):

Recall:
\[
y = \sqrt[3]{a} \implies a = y^3
\]
But \( a = t + \sqrt{t^2-1} \implies \sqrt{t^2 - 1} = a - t \implies t^2 - 1 = (a-t)^2 \)
Let’s instead work with the following relation.

Let’s cube both sides in the original variable:
\[
y^3 = \sqrt{x^2+1} + x
\implies y^3 - x = \sqrt{x^2+1}
\]
Now let’s cube again:
\[
(y^3 - x)^2 = x^2 + 1 \implies y^6 - 2x y^3 + x^2 = x^2 + 1
\]
\[
y^6 - 2x y^3 = 1
\implies 2x y^3 = y^6 - 1 \implies x = \frac{y^6 - 1}{2 y^3}
\]

Now find \( dx \) in terms of \( dy \):

\[
dx = \frac{d}{dy} \left( \frac{y^6 - 1}{2 y^3} \right) dy
\]
Let’s compute this derivative:
\[
\frac{d}{dy}\left( \frac{y^6 - 1}{2 y^3} \right) = \frac{6y^5 \cdot 2 y^3 - (y^6 - 1) \cdot 6 y^2}{4 y^6}
\]
But it's easier to use quotient rule:

Let’s let \( u = y^6 - 1 \), \( v = 2y^3 \)
\[
\frac{du}{dy} = 6 y^5,\qquad \frac{dv}{dy} = 6y^2
\]
\[
\frac{dx}{dy} = \frac{v \frac{du}{dy} - u \frac{dv}{dy}}{v^2}
= \frac{2y^3 \cdot 6y^5 - (y^6-1) \cdot 6y^2}{4y^6}
\]
\[
= \frac{12y^8 - 6y^8 + 6y^2}{4y^6}
= \frac{6y^8 + 6y^2}{4y^6}
= \frac{6(y^8 + y^2)}{4 y^6}
= \frac{3(y^8 + y^2)}{2 y^6}
= \frac{3y^2 (y^6 + 1)}{2 y^6}
= \frac{3(y^6 + 1)}{2 y^4}
\]

Therefore,
\[
dx = \frac{3(y^6 + 1)}{2 y^4} dy
\]

Recall, the integrand in terms of \( y \) is \( y - \frac{1}{y} \).

Now, what are the new integration limits?

At \( x = 0 \):

\[
y^3 = \sqrt{0^2 + 1} + 0 = 1 \implies y = 1
\]

At \( x=7 \):

\[
y^3 = \sqrt{7^2 + 1} + 7 = \sqrt{49+1} + 7 = \sqrt{50} + 7 = 5\sqrt{2} + 7
\implies y = (5\sqrt{2} + 7)^{1/3}
\]

Let’s denote \( A = (5\sqrt{2} + 7)^{1/3} \).

So we have,

\[
I = \int_{y=1}^{y=A} \left( y - \frac{1}{y} \right) \frac{3(y^6 + 1)}{2 y^4} dy
\]

Let’s expand the integrand:

\[
\left(y - \frac{1}{y}\right) \frac{3(y^6 + 1)}{2 y^4}
= \frac{3}{2} (y - \frac{1}{y}) \frac{y^6 + 1}{y^4}
= \frac{3}{2} \left( y \frac{y^6 + 1}{y^4} - \frac{1}{y} \frac{y^6 + 1}{y^4} \right)
= \frac{3}{2} \left( \frac{y^7 + y}{y^4} - \frac{y^6 + 1}{y^5} \right )
= \frac{3}{2} \left( y^3 + y^{-3} - y + y^{-5} \right )
\]

Let’s check this:

- \( y^7 / y^4 = y^3 \)
- \( y / y^4 = y^{-3} \)
- \( y^6 / y^5 = y \)
- \( 1 / y^5 = y^{-5} \)

Perfect.

So the new integrand is:

\[
\frac{3}{2} \left( y^3 + y^{-3} - y - y^{-5} \right )
\]

Thus,

\[
I = \frac{3}{2} \int_{1}^{A} \left( y^3 + y^{-3} - y - y^{-5} \right ) dy
\]

Let’s integrate term by term:

- \( \int y^3 dy = \frac{1}{4} y^4 \)
- \( \int y^{-3} dy = \frac{y^{-2}}{-2} = -\frac{1}{2} y^{-2} \)
- \( \int y dy = \frac{1}{2} y^2 \)
- \( \int y^{-5} dy = \frac{y^{-4}}{-4} = -\frac{1}{4} y^{-4} \)

Collecting these:

\[
I = \frac{3}{2} \left[ \frac{1}{4} y^4 - \frac{1}{2} y^{-2} - \frac{1}{2} y^2 + \frac{1}{4} y^{-4} \right ]_{y=1}^{y=A}
\]

Let’s factor out \( \frac{1}{4} \):

\[
I = \frac{3}{8} \left[ y^4 - 2 y^{-2} - 2 y^2 + y^{-4} \right ]_{1}^{A}
\]

Now,
\[
I = \frac{3}{8} \left[ (A^4 - 2A^{-2} - 2A^{2} + A^{-4}) - (1 - 2(1) - 2(1) + 1) \right ]
\]

Compute the lower bound:
\[
1 - 2(1) - 2(1) + 1 = 1 - 2 - 2 + 1 = (1+1) + (-2 - 2) = 2 - 4 = -2
\]

So,

\[
I = \frac{3}{8} \left[ A^4 - 2A^{-2} - 2A^{2} + A^{-4} + 2 \right ]
\]

Recall:

\[
A = (5 \sqrt{2} + 7)^{1/3}
\]

Let’s write \( A^{-2} = [(5\sqrt{2} + 7)^{1/3}]^{-2} = (5\sqrt{2} + 7)^{-2/3} \)

and similarly, \( A^2 = (5\sqrt{2} + 7)^{2/3} \), \( A^4 = (5\sqrt{2} + 7)^{4/3} \), \( A^{-4} = (5\sqrt{2} + 7)^{-4/3} \).

The exact answer is:

\[
I = \frac{3}{8} \left[ (5\sqrt{2} + 7)^{4/3} - 2 (5\sqrt{2} + 7)^{-2/3} - 2(5\sqrt{2} + 7)^{2/3} + (5\sqrt{2} + 7)^{-4/3} + 2 \right ]
\]

**Step 3: Numerical approximation**

Let’s compute:

- \( 5\sqrt{2} = 5 \times 1.4142135623730951 \approx 7.0710678118654755 \)
- \( 7.0710678118654755 + 7 = 14.071067811865476 \)
- \( A = (14.071067811865476)^{1/3} \)
- \( \log(14.071067811865476)/3 = \log(14.071067811865476, 10) / 3 \)
But let's compute the numbers directly (using a calculator):

First, \( A = (14.071067811865476)^{1/3} \):
- \( \ln(14.071067811865476) = 2.644431744186 \)
- \( \ln(A) = 2.644431744186/3 = 0.881477248062 \)
- \( A = \exp(0.881477248062) \approx 2.414213562 \)

But easier via direct computation:
- \( A = 14.071067811865476^{1/3} \)
- \( A \approx 2.414213562 \) (let’s check \( 2.414213562^3 \approx 14.0710678 \), yes)

So now:

- \( A = 2.414213562 \)
- \( A^{-2} = 2.414213562^{-2} \approx 0.1715728752 \)
- \( A^{2} = 2.414213562^2 \approx 5.828427125 \)
- \( A^{4} = (A^2)^2 \approx 5.828427125^2 \approx 33.99999999 \)
- \( A^{-4} = (A^{4})^{-1} \approx 0.02941176471 \)

Plug in:

- \( A^4 = 34.0 \)
- \( -2A^{-2} = -2 \times 0.1715728752 = -0.3431457504 \)
- \( -2A^2 = -2 \times 5.828427125 = -11.65685425 \)
- \( A^{-4} = 0.02941176471 \)
- \( +2 \)

Sum:
\[
S = 34.0 - 0.3431457504 - 11.65685425 + 0.02941176471 + 2
\]

Compute step by step:

- \( 34.0 - 0.3431457504 = 33.65685425 \)
- \( 33.65685425 - 11.65685425 = 22.0 \)
- \( 22.0 + 0.02941176471 = 22.02941176 \)
- \( 22.02941176 + 2 = 24.02941176 \)

Now multiply by \( \frac{3}{8} \):

\( \frac{3}{8} \approx 0.375 \)
\( 0.375 \times 24.02941176 = 9.01102941 \)

Rounded to \(10\) decimal places: \(9.0110294118\).

**Final answer:**

```json
{"answer": "\\frac{3}{8} \\left[ (5\\sqrt{2}+7)^{4/3} - 2(5\\sqrt{2}+7)^{-2/3} - 2(5\\sqrt{2}+7)^{2/3} + (5\\sqrt{2}+7)^{-4/3} + 2 \\right ]", "numerical_answer": "9.0110294118"}
```