# Evaluating $\int\limits_0^1\arccos xJ_0(ax)dx$

I'll solve this definite integral involving the Bessel function $J_0(ax)$ and $\arccos x$.

## Step 1: Initial setup
Let's denote the integral as:
$$I(a) = \int\limits_0^1\arccos xJ_0(ax)dx$$

Where $J_0(ax)$ is the Bessel function of the first kind of order 0.

## Step 2: Integration by parts
I'll use integration by parts with:
- $u = \arccos x$
- $dv = J_0(ax)dx$

This gives:
$$I(a) = \arccos x \int J_0(ax)dx - \int\left(\frac{d}{dx}\arccos x\right)\left(\int J_0(ax)dx\right)dx$$

## Step 3: Working with the Bessel function
We know that $\int J_0(ax)dx = \frac{1}{a}J_1(ax)$, where $J_1$ is the Bessel function of first kind of order 1.

Also, $\frac{d}{dx}\arccos x = -\frac{1}{\sqrt{1-x^2}}$

Substituting:
$$I(a) = \arccos x \cdot \frac{1}{a}J_1(ax) - \int\left(-\frac{1}{\sqrt{1-x^2}}\right)\left(\frac{1}{a}J_1(ax)\right)dx$$

$$I(a) = \frac{\arccos x \cdot J_1(ax)}{a} + \frac{1}{a}\int\frac{J_1(ax)}{\sqrt{1-x^2}}dx$$

## Step 4: Evaluating the first term at boundaries
Evaluating the first term at the limits $x=0$ and $x=1$:

At $x=0$: $\arccos(0) = \frac{\pi}{2}$ and $J_1(0) = 0$
At $x=1$: $\arccos(1) = 0$ and $J_1(a)$ is some value

So the first term becomes:
$$\left[\frac{\arccos x \cdot J_1(ax)}{a}\right]_0^1 = \frac{0 \cdot J_1(a)}{a} - \frac{\frac{\pi}{2} \cdot 0}{a} = 0$$

## Step 5: Handling the remaining integral
The remaining integral is:
$$\frac{1}{a}\int_0^1\frac{J_1(ax)}{\sqrt{1-x^2}}dx$$

This is a special form that evaluates to:
$$\frac{1}{a}\int_0^1\frac{J_1(ax)}{\sqrt{1-x^2}}dx = \frac{1}{a^2}(1-\cos a)$$

## Step 6: Final result
Therefore:
$$I(a) = \frac{1-\cos a}{a^2}$$

This is our exact answer.

## Step 7: Numerical approximation
For a numerical approximation, I need a specific value of $a$. Since none was provided, I'll express the numerical value in terms of $a$:

For any specific value of $a ≠ 0$, the numerical approximation would be:
$$\frac{1-\cos a}{a^2}$$

If we were to take $a = 1$ as an example, the numerical value would be:
$\frac{1-\cos(1)}{1^2} = 1-\cos(1) ≈ 0.4596976941$

{"answer": "\\frac{1-\\cos a}{a^2}", "numerical_answer": "\\frac{1-\\cos a}{a^2}"}