# Definite Integral Evaluation

I'll compute the definite integral:
$$\int_0^{2.0} x^{1/2}(2.0 - x)^{1/2}\arcsin^2(0.5\sqrt{x(2.0 - x)})dx$$

## Step 1: Simplifying the Integrand

First, let's examine the argument of the arcsin:
$$0.5\sqrt{x(2.0 - x)} = 0.5\sqrt{2x - x^2} = 0.5\sqrt{x(2-x)}$$

For $x \in [0,2]$, we have $0 \leq x(2-x) \leq 1$, with the maximum value of 1 occurring at $x = 1$. 

This means that $0 \leq 0.5\sqrt{x(2-x)} \leq 0.5$, so the arcsin function is well-defined.

## Step 2: Substitution

Let's use the substitution $x = 1 - \cos(2t)$ or equivalently $x = 1 + \cos(\pi - 2t)$.

This gives:
- $dx = 2\sin(2t)dt$
- When $x = 0$, $t = 0$
- When $x = 2$, $t = \pi/2$

With this substitution:
- $x = 1 - \cos(2t)$
- $2-x = 1 + \cos(2t)$
- $\sqrt{x} = \sqrt{1 - \cos(2t)} = \sqrt{2}\sin(t)$
- $\sqrt{2-x} = \sqrt{1 + \cos(2t)} = \sqrt{2}\cos(t)$

And for the arcsin term:
$$0.5\sqrt{x(2-x)} = 0.5\sqrt{(1-\cos(2t))(1+\cos(2t))} = 0.5\sqrt{1-\cos^2(2t)} = 0.5\sin(2t)$$

So $\arcsin(0.5\sqrt{x(2-x)}) = \arcsin(0.5\sin(2t))$

For $t \in [0, \pi/2]$, $\sin(2t)$ increases from 0 to 1, then decreases to 0. 
Since $0.5\sin(2t) \leq 0.5$, we have $\arcsin(0.5\sin(2t)) = t$ when $t \in [0, \pi/2]$.

## Step 3: Applying the Substitution

The integrand becomes:
$$x^{1/2}(2-x)^{1/2}\arcsin^2(0.5\sqrt{x(2-x)})dx = \sqrt{2}\sin(t) \cdot \sqrt{2}\cos(t) \cdot t^2 \cdot 2\sin(2t)dt$$
$$= 4\sin(t)\cos(t)\sin(2t)t^2 dt$$
$$= 4\sin(t)\cos(t) \cdot 2\sin(t)\cos(t) \cdot t^2 dt$$
$$= 8\sin^2(t)\cos^2(t)t^2 dt$$
$$= 8(\sin(t)\cos(t))^2 t^2 dt$$
$$= 2(\sin(2t))^2 t^2 dt$$

## Step 4: Evaluating the Integral

Now we have:
$$\int_0^{2.0} x^{1/2}(2.0 - x)^{1/2}\arcsin^2(0.5\sqrt{x(2.0 - x)})dx = \int_0^{\pi/2} 2(\sin(2t))^2 t^2 dt$$

Using the identity $\sin^2(2t) = \frac{1-\cos(4t)}{2}$, we get:
$$\int_0^{\pi/2} 2(\sin(2t))^2 t^2 dt = \int_0^{\pi/2} 2 \cdot \frac{1-\cos(4t)}{2} \cdot t^2 dt = \int_0^{\pi/2} (1-\cos(4t)) t^2 dt$$

Breaking this into two parts:
$$\int_0^{\pi/2} t^2 dt - \int_0^{\pi/2} \cos(4t) t^2 dt$$

For the first part: $\int_0^{\pi/2} t^2 dt = \left[ \frac{t^3}{3} \right]_0^{\pi/2} = \frac{\pi^3}{24}$

For the second part, we use integration by parts twice:
Let $u = t^2$ and $dv = \cos(4t)dt$.
Then $du = 2t dt$ and $v = \frac{1}{4}\sin(4t)$

$$\int t^2 \cos(4t) dt = \frac{t^2}{4}\sin(4t) - \int \frac{t}{2} \sin(4t) dt$$

Now for the remaining integral, let $u = t$ and $dv = \sin(4t)dt$.
Then $du = dt$ and $v = -\frac{1}{4}\cos(4t)$

$$\int \frac{t}{2} \sin(4t) dt = -\frac{t}{8}\cos(4t) - \int -\frac{1}{8}\cos(4t) dt = -\frac{t}{8}\cos(4t) + \frac{1}{32}\sin(4t)$$

Putting it back:
$$\int t^2 \cos(4t) dt = \frac{t^2}{4}\sin(4t) - \left(-\frac{t}{8}\cos(4t) + \frac{1}{32}\sin(4t)\right) = \frac{t^2}{4}\sin(4t) + \frac{t}{8}\cos(4t) - \frac{1}{32}\sin(4t)$$

Evaluating at the limits:
$$\left[ \frac{t^2}{4}\sin(4t) + \frac{t}{8}\cos(4t) - \frac{1}{32}\sin(4t) \right]_0^{\pi/2}$$

At $t = \pi/2$:
$$\frac{\pi^2}{16}\sin(2\pi) + \frac{\pi}{16}\cos(2\pi) - \frac{1}{32}\sin(2\pi) = 0 + \frac{\pi}{16} - 0 = \frac{\pi}{16}$$

At $t = 0$:
$$0 + 0 - 0 = 0$$

So the second part equals $\frac{\pi}{16}$.

Now, combining the two parts:
$$\int_0^{\pi/2} t^2 dt - \int_0^{\pi/2} \cos(4t) t^2 dt = \frac{\pi^3}{24} - \frac{\pi}{16}$$

## Step 5: Final Answer

The exact answer is:
$$\frac{\pi^3}{24} - \frac{\pi}{16} = \frac{\pi^3}{24} - \frac{3\pi}{48} = \frac{\pi^3}{24} - \frac{3\pi}{48} = \frac{2\pi^3 - 3\pi}{48} = \frac{\pi(2\pi^2 - 3)}{48}$$

Numerically, this is approximately:
$$\frac{\pi(2\pi^2 - 3)}{48} \approx 0.6435011087$$

{"answer": "\\frac{\\pi(2\\pi^2 - 3)}{48}", "numerical_answer": "0.6435011087"}