To compute the definite integral \(\int_0^1 \frac{\ln x \ln \frac{2+x}{2-x}}{x} \, dx\), we proceed as follows:

1. **Analytical Solution**:
   - Expand the logarithm term \(\ln \frac{2+x}{2-x}\) using properties of logarithms:
     \[
     \ln \frac{2+x}{2-x} = \ln(2+x) - \ln(2-x)
     \]
   - Split the integral into two parts:
     \[
     \int_0^1 \frac{\ln x \ln(2+x)}{x} \, dx - \int_0^1 \frac{\ln x \ln(2-x)}{x} \, dx
     \]
   - Use series expansions for \(\ln(2+x)\) and \(\ln(2-x)\):
     \[
     \ln(2+x) = \ln 2 + \sum_{k=1}^\infty (-1)^{k+1} \frac{x^k}{k 2^k}, \quad \ln(2-x) = \ln 2 - \sum_{k=1}^\infty \frac{x^k}{k 2^k}
     \]
   - Subtract the series and simplify, leading to:
     \[
     \ln \frac{2+x}{2-x} = 2 \sum_{k=0}^\infty \frac{(x/2)^{2k+1}}{2k+1}
     \]
   - Substitute back into the integral and interchange summation and integration:
     \[
     \int_0^1 \frac{\ln x}{x} \cdot 2 \sum_{k=0}^\infty \frac{(x/2)^{2k+1}}{2k+1} \, dx
     \]
   - Simplify and integrate term-by-term using \(\int_0^1 x^{2k} \ln x \, dx = -\frac{1}{(2k+1)^2}\):
     \[
     -2 \sum_{k=0}^\infty \frac{1}{(2k+1)^3 4^k}
     \]

2. **Numerical Approximation**:
   - Compute the series \(\sum_{n=0}^\infty \frac{1}{4^n (2n+1)^3}\) numerically up to sufficient terms for precision:
     \[
     \text{Numerical value} \approx -1.0098110630
     \]

The final answer is:

{"answer": "-\\sum_{n=0}^{\\infty} \\frac{1}{4^{n} (2n+1)^3}", "numerical_answer": "-1.0098110630"}