Let's follow the requested steps for the definite integral:
\[
I = \int_0^2 x^{-1/2} H_3 \left(\sqrt[4]{x(2-x)}\right) dx,
\]
where \( H_3(x) \) is the third Hermite polynomial. Recall that \( H_3(x) = 8x^3 - 12x \).

### Step 1: Replace \( H_3 \) and expand the integrand

Let \( y = \sqrt[4]{x(2-x)} \).

So,
\[
H_3(y) = 8y^3 - 12y
\]

Plug into the integral:
\[
I = \int_0^2 x^{-1/2} [8y^3 - 12y] dx
   = 8 \int_0^2 x^{-1/2} y^3 dx - 12 \int_0^2 x^{-1/2} y dx
\]

Since \( y = (x(2-x))^{1/4} \):
- \( y^3 = (x(2-x))^{3/4} \)
- \( y = (x(2-x))^{1/4} \)

Thus, 
\[
I = 8 \int_0^2 x^{-1/2} [x(2-x)]^{3/4} dx
    - 12 \int_0^2 x^{-1/2} [x(2-x)]^{1/4} dx
\]

Let's call them \( I_1 \) and \( I_2 \):
\[
I_1 = \int_0^2 x^{-1/2} [x(2-x)]^{3/4} dx
\]
\[
I_2 = \int_0^2 x^{-1/2} [x(2-x)]^{1/4} dx
\]

### Step 2: Make a substitution

Let \( x = 2 \sin^2 \theta \), \( 0 \leq \theta \leq \frac{\pi}{2} \).
Then \( dx = 4 \sin \theta \cos \theta d\theta = 2 \sin 2\theta d\theta \).

Compute expressions:

- \( x^{-1/2} = (2 \sin^2 \theta)^{-1/2} = \frac{1}{\sqrt{2} \sin \theta} \)
- \( x(2 - x) = 2 \sin^2 \theta (2 - 2 \sin^2 \theta) = 4 \sin^2 \theta \cos^2 \theta = (\sin 2\theta)^2 \)
- Therefore, \( [x(2-x)]^{p/4} = [\sin 2\theta]^{p/2} \)

Let's compute \( I_1 \):

#### For \( I_1 \):

- \( p = 3 \), so exponent is \( 3/4 \), so we get \( [x(2-x)]^{3/4} = [\sin 2\theta]^{3/2} \)

So,
\[
I_1 = \int_0^2 x^{-1/2} [x(2-x)]^{3/4} dx 
= \int_{\theta=0}^{\pi/2} \frac{1}{\sqrt{2} \sin \theta} \cdot [\sin 2\theta]^{3/2} \cdot 2 \sin 2\theta d\theta
\]

Now,
- \( [\sin 2\theta]^{3/2} \cdot \sin 2\theta = [\sin 2\theta]^{5/2} \)

So:
\[
I_1 = \int_0^{\pi/2} \frac{1}{\sqrt{2} \sin \theta} \cdot [\sin 2\theta]^{3/2} \cdot 2 \sin 2\theta d\theta
= \frac{2}{\sqrt{2}} \int_0^{\pi/2} \frac{ [\sin 2\theta]^{5/2} }{\sin \theta} d\theta
\]
Recall \( \sin 2\theta = 2 \sin\theta \cos\theta \), so \( [\sin 2\theta]^{5/2} = [2 \sin\theta \cos\theta]^{5/2} = 2^{5/2} [\sin\theta]^{5/2} [\cos\theta]^{5/2} \)

So,
\[
I_1 = \sqrt{2} \int_0^{\pi/2} \frac{2^{5/2} [\sin\theta]^{5/2} [\cos\theta]^{5/2} }{ \sin\theta } d\theta
= \sqrt{2} \cdot 2^{5/2} \int_0^{\pi/2} [\sin\theta]^{3/2} [\cos\theta]^{5/2} d\theta
\]

Calculate \( \sqrt{2} \cdot 2^{5/2} = 2^{1/2} \cdot 2^{5/2} = 2^{(1/2+5/2)} = 2^{3} = 8 \)

So,
\[
I_1 = 8 \int_0^{\pi/2} [\sin\theta]^{3/2} [\cos\theta]^{5/2} d\theta
\]

#### For \( I_2 \):

Similarly, for \( p=1 \):

\[
I_2 = \int_0^2 x^{-1/2} [x(2-x)]^{1/4} dx 
= \int_0^{\pi/2} \frac{1}{\sqrt{2} \sin \theta} \cdot [\sin 2\theta]^{1/2} \cdot 2 \sin 2\theta d\theta
= \frac{2}{\sqrt{2}} \int_0^{\pi/2} \frac{ [\sin 2\theta]^{3/2} }{ \sin\theta } d\theta
\]

Now,

\[
[\sin 2\theta]^{3/2} = [2 \sin\theta \cos\theta]^{3/2} = 2^{3/2} [\sin\theta]^{3/2} [\cos\theta]^{3/2}
\]

Therefore,

\[
I_2 = \sqrt{2} \int_0^{\pi/2} 2^{3/2} [\sin\theta]^{3/2} [\cos\theta]^{3/2} / \sin\theta d\theta
= \sqrt{2} \cdot 2^{3/2} \int_0^{\pi/2} [\sin\theta]^{1/2} [\cos\theta]^{3/2} d\theta
\]
\( \sqrt{2} \cdot 2^{3/2} = 2^{1/2 + 3/2} = 2^2 = 4 \)

Therefore,

\[
I_2 = 4 \int_0^{\pi/2} [\sin\theta]^{1/2} [\cos\theta]^{3/2} d\theta
\]

### Step 3: Substitute back into the original expression

Recall
\[
I = 8I_1 - 12I_2
\]
Substitute the above,
\[
I = 8 \left( 8 \int_0^{\pi/2} [\sin\theta]^{3/2} [\cos\theta]^{5/2} d\theta \right )
  - 12 \left( 4 \int_0^{\pi/2} [\sin\theta]^{1/2} [\cos\theta]^{3/2} d\theta \right )
\]
\[
I = 64 \int_0^{\pi/2} [\sin\theta]^{3/2} [\cos\theta]^{5/2} d\theta
   - 48 \int_0^{\pi/2} [\sin\theta]^{1/2} [\cos\theta]^{3/2} d\theta
\]

Write both in terms of the Beta function:

\[
\int_0^{\pi/2} (\sin\theta)^{a - 1} (\cos\theta)^{b - 1} d\theta
= \frac{1}{2} B \left(\frac{a}{2}, \frac{b}{2}\right)
\]

So,

- For the first term: \( a = 3/2 + 1 = 5/2 \), \( b = 5/2 + 1 = 7/2 \)
  (Wait: But in the standard form, the exponents are \(a - 1\) and \(b - 1\). For us,
   so \( [\sin\theta]^{3/2} \) means \( a - 1 = 3/2 \Rightarrow a = 5/2 \), and \( [\cos\theta]^{5/2} \) so \(b = 7/2\).

- For the second term: \( a = 1/2 + 1 = 3/2 \), \( b = 3/2 + 1 = 5/2 \), so \(a = 3/2\), \(b = 5/2\).

Thus,

\[
I = 64 \cdot \int_0^{\pi/2} (\sin\theta)^{3/2} (\cos\theta)^{5/2} d\theta
   - 48 \cdot \int_0^{\pi/2} (\sin\theta)^{1/2} (\cos\theta)^{3/2} d\theta
\]
\[
= 64 \cdot \frac{1}{2} B\Big(\frac{5}{4}, \frac{7}{4}\Big)
  - 48 \cdot \frac{1}{2} B\Big(\frac{3}{4}, \frac{5}{4}\Big)
\]
\[
= 32 B\Big(\frac{5}{4}, \frac{7}{4}\Big) - 24 B\Big(\frac{3}{4}, \frac{5}{4}\Big)
\]

Now, recall that the Beta function can be rewritten in terms of gamma functions:
\[
B(a,b) = \frac{\Gamma(a)\Gamma(b)}{\Gamma(a+b)}
\]

So,
\[
I = 32 \cdot \frac{\Gamma(5/4)\Gamma(7/4)}{\Gamma(3)}
  - 24 \cdot \frac{\Gamma(3/4)\Gamma(5/4)}{\Gamma(2)}
\]

Now, \( \Gamma(2) = 1! = 1 \), \( \Gamma(3) = 2! = 2 \).

Thus,
\[
I = 32 \cdot \frac{\Gamma(5/4)\Gamma(7/4)}{2} - 24 \cdot \Gamma(3/4)\Gamma(5/4)
\]
\[
= 16 \Gamma\left(\frac{5}{4}\right)\Gamma\left(\frac{7}{4}\right)
   - 24 \Gamma\left(\frac{3}{4}\right)\Gamma\left(\frac{5}{4}\right)
\]
\[
= \Gamma\left(\frac{5}{4}\right) \left[ 16 \Gamma\left(\frac{7}{4}\right) - 24 \Gamma\left(\frac{3}{4}\right) \right]
\]

### Step 4: Analytical answer in LaTeX

\[
\boxed{
I = 16 \, \Gamma\left(\frac{5}{4}\right) \Gamma\left(\frac{7}{4}\right)
    - 24 \, \Gamma\left(\frac{3}{4}\right) \Gamma\left(\frac{5}{4}\right)
}
\]

Or, factoring as above,

\[
\boxed{
I = \Gamma\left(\frac{5}{4}\right)
\left[ 16 \Gamma\left(\frac{7}{4}\right) - 24 \Gamma\left(\frac{3}{4}\right) \right]
}
\]

### Step 5: Numerical Approximation

We need:
- \( \Gamma(3/4) \approx 1.225416703 \)
- \( \Gamma(5/4) \approx 0.9064024771 \)
- \( \Gamma(7/4) \approx 0.9181687424 \)

Now,

First term:
\[
16 \cdot \Gamma(5/4) \cdot \Gamma(7/4) \approx 16 \times 0.9064024771 \times 0.9181687424
\]
Calculate \( 0.9064024771 \times 0.9181687424 \approx 0.8319150123 \)
Thus,
\[
16 \times 0.8319150123 = 13.310640197
\]

Second term:
\[
24 \cdot \Gamma(3/4) \cdot \Gamma(5/4) \approx 24 \times 1.225416703 \times 0.9064024771
\]
Calculate \( 1.225416703 \times 0.9064024771 \approx 1.110312173 \)
Thus,
\[
24 \times 1.110312173 \approx 26.64749214
\]

Now, subtract:
\[
I \approx 13.310640197 - 26.64749214 = -13.33685195
\]

**Rounded to 10 decimal places:**

\[
I \approx -13.3368519500
\]

### Final JSON format

```json
{"answer": "16\\, \\Gamma\\left(\\tfrac{5}{4}\\right) \\Gamma\\left(\\tfrac{7}{4}\\right) - 24\\, \\Gamma\\left(\\tfrac{3}{4}\\right)\\Gamma\\left(\\tfrac{5}{4}\\right)", "numerical_answer": "-13.3368519500"}
```