To solve the definite integral \(\int_{64}^{729} \frac{x^{1/2}}{x^{1/2} - x^{1/3}} \, dx\), we will follow the steps outlined:

### Step 1: Simplify the integrand

First, let's simplify the integrand \(\frac{x^{1/2}}{x^{1/2} - x^{1/3}}\).

Let \(u = x^{1/6}\). Then \(x = u^6\) and \(dx = 6u^5 \, du\).

Rewrite the integrand in terms of \(u\):
\[
x^{1/2} = (u^6)^{1/2} = u^3
\]
\[
x^{1/3} = (u^6)^{1/3} = u^2
\]

Thus, the integrand becomes:
\[
\frac{u^3}{u^3 - u^2} = \frac{u^3}{u^2(u - 1)} = \frac{u}{u - 1}
\]

### Step 2: Integrate the simplified expression

Now, we need to integrate \(\frac{u}{u - 1}\) with respect to \(u\):
\[
\int \frac{u}{u - 1} \, du
\]

We can split this into two simpler integrals:
\[
\int \frac{u}{u - 1} \, du = \int \left(1 + \frac{1}{u - 1}\right) \, du = \int 1 \, du + \int \frac{1}{u - 1} \, du
\]

Integrating each term separately:
\[
\int 1 \, du = u
\]
\[
\int \frac{1}{u - 1} \, du = \ln|u - 1|
\]

So, the integral is:
\[
u + \ln|u - 1| + C
\]

### Step 3: Substitute back and evaluate the definite integral

Substitute \(u = x^{1/6}\) back into the expression:
\[
x^{1/6} + \ln|x^{1/6} - 1| + C
\]

Evaluate this from \(x = 64\) to \(x = 729\):
\[
\left[ x^{1/6} + \ln|x^{1/6} - 1| \right]_{64}^{729}
\]

Calculate the values at the bounds:
For \(x = 729\):
\[
729^{1/6} = 3
\]
\[
\ln|3 - 1| = \ln 2
\]

For \(x = 64\):
\[
64^{1/6} = 2
\]
\[
\ln|2 - 1| = \ln 1 = 0
\]

So, the definite integral is:
\[
(3 + \ln 2) - (2 + 0) = 3 + \ln 2 - 2 = 1 + \ln 2
\]

### Step 4: Numerical approximation

The numerical approximation of \(1 + \ln 2\) is:
\[
1 + \ln 2 \approx 1 + 0.69314718056 = 1.69314718056
\]

### Final Answer

\[
\boxed{
\begin{aligned}
\text{"answer": "1 + \ln 2",} \\
\text{"numerical_answer": "1.6931471806"}
\end{aligned}
}
\]