<think>
Okay, let's see. I need to compute the definite integral from 0 to 2 of x^(-1/2)(2 - x)^(-1/2) cosh(1 * sqrt(x(2 - x))) dx. Hmm, that looks a bit complicated, but maybe there's a substitution that can simplify it.

First, let me write down the integral again to make sure I have it right:

∫₀² x^(-1/2) (2 - x)^(-1/2) cosh(√(x(2 - x))) dx

The integrand has x and (2 - x) terms raised to the -1/2 power, and the argument of the cosh is the square root of x(2 - x). That square root inside the cosh might be a clue. Maybe a substitution that simplifies the expression under the square root.

Let me consider substituting t = x - 1. That might center the interval around 0, since x goes from 0 to 2. If t = x - 1, then x = t + 1, and when x=0, t=-1; x=2, t=1. But the limits would be from -1 to 1. Hmm, not sure if that helps. Alternatively, maybe a trigonometric substitution?

Wait, the product x(2 - x) is similar to the expression 1 - (x - 1)^2. Let me check:

x(2 - x) = 2x - x² = -(x² - 2x) = -(x² - 2x +1 -1) = -(x -1)^2 +1 = 1 - (x -1)^2. Yes! So sqrt(x(2 -x)) = sqrt(1 - (x -1)^2). That looks like the equation of a circle. Maybe a substitution using sine or cosine.

Let me try substituting u = x -1. Then du = dx, and when x=0, u=-1; x=2, u=1. The integral becomes:

∫_{-1}^{1} (u +1)^(-1/2) (1 - u)^(-1/2) cosh(sqrt(1 - u²)) du

Wait, (u +1) is (x) and (1 - u) is (2 - x). So the product (u +1)(1 - u) = (1 - u²). Therefore, the terms (u +1)^(-1/2) (1 - u)^(-1/2) = (1 - u²)^(-1/2). So the integrand becomes (1 - u²)^(-1/2) cosh(sqrt(1 - u²)) du, integrated from -1 to 1.

So the integral simplifies to:

∫_{-1}^{1} [1 / sqrt(1 - u²)] cosh(sqrt(1 - u²)) du

Hmm, that seems more manageable. Also, the integrand is even because cosh is even and sqrt(1 - u²) is even. So we can write this as 2 times the integral from 0 to 1.

So, 2 ∫₀¹ [1 / sqrt(1 - u²)] cosh(sqrt(1 - u²)) du

Now, let's make another substitution. Let’s set t = sqrt(1 - u²). Then t² = 1 - u². Differentiating both sides: 2t dt = -2u du ⇒ u du = -t dt. But we need to express du in terms of dt. Let's solve for du:

From u² = 1 - t² ⇒ u = sqrt(1 - t²). Then, du = (-t)/sqrt(1 - t²) dt. Wait, maybe this substitution complicates things. Let me try a different approach.

Alternatively, let’s set θ such that u = sinθ. Then, when u=0, θ=0; u=1, θ=π/2. Then, sqrt(1 - u²) = cosθ, and du = cosθ dθ. Let's substitute:

Then, the integral becomes:

2 ∫₀^{π/2} [1 / sqrt(1 - sin²θ)] cosh(cosθ) * cosθ dθ

But sqrt(1 - sin²θ) is cosθ, so [1 / cosθ] * cosh(cosθ) * cosθ dθ = cosh(cosθ) dθ. Therefore, the integral simplifies to:

2 ∫₀^{π/2} cosh(cosθ) dθ

Hmm, interesting. So now the integral is 2 times the integral of cosh(cosθ) from 0 to π/2. But how do I compute ∫ cosh(cosθ) dθ? That doesn't look straightforward. Maybe there's a series expansion for cosh(cosθ) that can be integrated term by term?

Recall that cosh(z) = Σ_{n=0}^∞ [z^{2n} / (2n)!]. So, cosh(cosθ) = Σ_{n=0}^∞ [cos^{2n}θ / (2n)!]. Then, integrating term by term:

∫₀^{π/2} cosh(cosθ) dθ = Σ_{n=0}^∞ [1/(2n)!] ∫₀^{π/2} cos^{2n}θ dθ

The integrals ∫₀^{π/2} cos^{2n}θ dθ are known and can be expressed using the beta function or the gamma function. Specifically, ∫₀^{π/2} cos^{2n}θ dθ = (π/2) * ( (2n)! ) / (4^n (n!)^2 )

So substituting back:

Σ_{n=0}^∞ [1/(2n)!] * (π/2) * ( (2n)! ) / (4^n (n!)^2 ) ) = (π/2) Σ_{n=0}^∞ [1 / (4^n (n!)^2 ) ]

But the sum Σ_{n=0}^∞ [ (1/4^n) / (n!)^2 ) ] is known. Wait, that's the modified Bessel function of the first kind I_0(1). Because I_0(z) = Σ_{n=0}^∞ [ (z/2)^{2n} / (n!)^2 ) ].

So, if we set z = 1, then I_0(1) = Σ_{n=0}^∞ [ (1/2)^{2n} / (n!)^2 ) ] = Σ_{n=0}^∞ [1/(4^n (n!)^2 ) ]

Therefore, the sum is I_0(1). Therefore, the integral becomes:

(π/2) * I_0(1)

Therefore, the original integral is 2 * (π/2) * I_0(1) = π I_0(1)

So the exact answer is π times the modified Bessel function of the first kind of order 0 evaluated at 1. So, π I_0(1).

Now, for the numerical approximation. The modified Bessel function I_0(1) can be calculated numerically. Let me recall its value. From tables or computational tools, I_0(1) ≈ 1.266065878. Let me verify this.

Alternatively, compute the sum Σ_{n=0}^∞ 1/(4^n (n!)^2 ). Let's compute the first few terms:

n=0: 1/(1*1) = 1

n=1: 1/(4*1) = 0.25

n=2: 1/(16*4) = 1/64 ≈ 0.015625

n=3: 1/(64*36) ≈ 0.000434

n=4: 1/(256*576) ≈ 0.0000068

Adding these up: 1 + 0.25 = 1.25; +0.015625 = 1.265625; +0.000434 ≈ 1.266059; +0.0000068 ≈ 1.2660658. So the sum converges to approximately 1.266065878. So I_0(1) ≈ 1.266065878.

Therefore, the integral is π * 1.266065878 ≈ 3.1415926536 * 1.266065878 ≈ Let's compute this:

First, 3 * 1.266065878 ≈ 3.798197634

0.1415926536 * 1.266065878 ≈

0.1 * 1.266065878 ≈ 0.1266065878

0.0415926536 * 1.266065878 ≈

0.04 * 1.266065878 ≈ 0.050642635

0.0015926536 * 1.266065878 ≈ ~0.002019

Adding these: 0.1266065878 + 0.050642635 ≈ 0.1772492228 + 0.002019 ≈ 0.1792682228

Total approximation: 3.798197634 + 0.1792682228 ≈ 3.9774658568

But let me use a calculator for more precision. π ≈ 3.141592653589793. Multiply by 1.266065878:

3.141592653589793 * 1.266065878 ≈

Let me compute step by step:

1.266065878 * 3 = 3.798197634

1.266065878 * 0.141592653589793 ≈

First, 1.1 * 0.141592653589793 ≈ 0.155751919

0.166065878 * 0.141592653589793 ≈

0.1 * 0.141592653589793 ≈ 0.014159265

0.066065878 * 0.141592653589793 ≈

Approx 0.06 * 0.141592653589793 ≈ 0.008495559

0.006065878 * 0.141592653589793 ≈ ~0.000858

Adding these: 0.014159265 + 0.008495559 ≈ 0.022654824 + 0.000858 ≈ 0.023512824

So total for 0.166065878 part: ~0.023512824

Adding to the 0.155751919: 0.155751919 + 0.023512824 ≈ 0.179264743

So total 3.798197634 + 0.179264743 ≈ 3.977462377

So approximately 3.977462377. Rounded to 10 decimal places, that's 3.9774623770. Let me check with a calculator. Alternatively, use known value of π I_0(1). The exact value is π I_0(1), and I_0(1) is approximately 1.2660658777522604. So π * 1.2660658777522604 ≈ 3.141592653589793 * 1.2660658777522604 ≈

Using a calculator: 3.141592653589793 * 1.26606587775226 ≈

3.141592653589793 * 1 = 3.141592653589793

3.141592653589793 * 0.2 = 0.6283185307179586

3.141592653589793 * 0.06 = 0.1884955592153876

3.141592653589793 * 0.006 = 0.01884955592153876

3.141592653589793 * 0.00006587775226 ≈ approx 3.141592653589793 * 0.00006 = 0.000188495559, and the rest is negligible.

Adding up:

3.141592653589793 + 0.6283185307179586 = 3.7699111843077516

+0.1884955592153876 = 3.958406743523139

+0.01884955592153876 = 3.977256299444678

+0.000188495559 ≈ 3.977444794

But considering more precise multiplication, perhaps using a calculator:

π ≈ 3.141592653589793

I_0(1) ≈ 1.2660658777522604

Multiplying these:

3.141592653589793 * 1.2660658777522604 ≈

Let me compute 3.141592653589793 * 1.2660658777522604:

First, 3 * 1.2660658777522604 = 3.798197633256781

0.141592653589793 * 1.2660658777522604 ≈

0.1 * 1.2660658777522604 = 0.12660658777522604

0.041592653589793 * 1.2660658777522604 ≈

0.04 * 1.2660658777522604 = 0.050642635110090416

0.001592653589793 * 1.2660658777522604 ≈ ~0.002019

Adding these: 0.12660658777522604 + 0.050642635110090416 ≈ 0.17724922288531645 + 0.002019 ≈ 0.17926822288531645

Total: 3.798197633256781 + 0.17926822288531645 ≈ 3.977465856142097

So approximately 3.9774658561. Rounded to 10 decimal places, that's 3.9774658561. Let me check with an online calculator. Alternatively, if I use the known value of π I_0(1), which is a standard integral. Wait, but maybe there's another way to verify.

Alternatively, perhaps the integral can be expressed in terms of Bessel functions. Let me recall that integrals involving cosh(a cosθ) can be related to Bessel functions. Indeed, there is an integral representation of the modified Bessel function:

I_0(z) = (1/π) ∫₀^π e^{z cosθ} dθ

But in our case, we have ∫₀^{π/2} cosh(cosθ) dθ. Since cosh is the even part of the exponential function, we can write cosh(cosθ) = [e^{cosθ} + e^{-cosθ}]/2. But integrating from 0 to π/2:

∫₀^{π/2} cosh(cosθ) dθ = (1/2) [∫₀^{π/2} e^{cosθ} dθ + ∫₀^{π/2} e^{-cosθ} dθ ]

But the integral ∫₀^{π} e^{z cosθ} dθ = π I_0(z). So if we take z=1, then ∫₀^{π} e^{cosθ} dθ = π I_0(1). Therefore, ∫₀^{π/2} e^{cosθ} dθ = (1/2) ∫₀^{π} e^{cosθ} dθ = (π/2) I_0(1). Similarly, ∫₀^{π/2} e^{-cosθ} dθ = (π/2) I_0(1) as well, since cosθ is even and replacing θ by π - θ would give the same integral. Wait, maybe not. Let me check.

Wait, if we consider ∫₀^{π} e^{-cosθ} dθ, it's the same as ∫₀^{π} e^{cos(π - θ)} dθ), but maybe it's also equal to π I_0(1). Because I_0(z) is even in z. Wait, I_0(z) = I_0(-z). So ∫₀^{π} e^{-cosθ} dθ = π I_0(1). Therefore, ∫₀^{π/2} e^{-cosθ} dθ = (π/2) I_0(1). Therefore, the sum becomes:

(1/2) [ (π/2) I_0(1) + (π/2) I_0(1) ] = (1/2)(π I_0(1)) = π/2 I_0(1)

Wait, but earlier we had ∫₀^{π/2} cosh(cosθ) dθ = (1/2)[A + B], where A and B are the integrals of e^{cosθ} and e^{-cosθ} from 0 to π/2. But according to the integral representation, A = B = (π/2) I_0(1). Therefore, the sum is (1/2)( (π/2 I_0(1)) + (π/2 I_0(1)) ) = (1/2)(π I_0(1)) = π/2 I_0(1). Therefore, but earlier we had:

Original integral after substitution was 2 * ∫₀^{π/2} cosh(cosθ) dθ = 2 * (π/2) I_0(1) = π I_0(1). Which matches our previous result. So that's correct.

Therefore, the exact answer is π I_0(1), and the value is approximately 3.9774632605 (but earlier calculation gave ~3.9774658561). Let me check with a calculator for more precision.

Looking up the value of I_0(1):

According to Wolfram Alpha, I_0(1) ≈ 1.2660658777522604. Then π * 1.2660658777522604 ≈ 3.9774632605. Rounded to 10 decimal places, that's 3.9774632605. Wait, but my previous step-by-step calculation gave approximately 3.9774658561. There's a slight discrepancy here. Let me check with precise multiplication.

Using more precise calculation:

1.2660658777522604 * π:

π ≈ 3.1415926535897932384626433832795

1.2660658777522604 * 3.1415926535897932384626433832795

Let me compute this using a calculator:

1.2660658777522604 * 3.141592653589793 ≈ 3.977463260509082

So rounded to 10 decimal places, that's 3.9774632605.

Therefore, the numerical approximation is approximately 3.9774632605.

So the exact answer is π I_0(1), which can be written in LaTeX as \pi I_0}(1), but need to check the Bessel function notation. The standard notation is I_0(1), so the exact answer is \pi I_0(1), which in LaTeX is \pi I_0(1). However, sometimes it's written with a subscript, so \pi I_0(1).

Therefore, the final answer is {"answer": "\pi I_0(1)", "numerical_answer": "3.9774632605"}.

But wait, let me confirm if there's a more simplified exact form. Sometimes integrals involving Bessel functions can be expressed in terms of other special functions, but in this case, the result is indeed π times the modified Bessel function of the first kind of order 0 at 1. There's no simpler elementary form for this integral, so the exact answer is π I₀(1), which in LaTeX is \pi I_0(1).

Yes, that's correct. So the JSON output should be:

{"answer": "\pi I_0(1)", "numerical_answer": "3.9774632605"}
</think>

{"answer": "\pi I_0(1)", "numerical_answer": "3.9774632605"}