# Evaluating $\int_{\frac18}^{\frac14}\frac{\ln(2x)\ln(4x)\ln(8x)}x\:\mathrm{d}x$

## Step 1: Rewrite the logarithms in terms of $\ln(x)$

First, I'll use the logarithm properties to rewrite each term:
- $\ln(2x) = \ln(2) + \ln(x)$
- $\ln(4x) = \ln(4) + \ln(x) = \ln(2^2) + \ln(x) = 2\ln(2) + \ln(x)$
- $\ln(8x) = \ln(8) + \ln(x) = \ln(2^3) + \ln(x) = 3\ln(2) + \ln(x)$

## Step 2: Expand the product

Let's multiply out these expressions:
$\ln(2x)\ln(4x)\ln(8x) = [\ln(2) + \ln(x)][2\ln(2) + \ln(x)][3\ln(2) + \ln(x)]$

This gives us:
$[\ln(2) + \ln(x)][2\ln(2) + \ln(x)][3\ln(2) + \ln(x)]$

Expanding this triple product:
$[\ln(2) + \ln(x)][6\ln^2(2) + 5\ln(2)\ln(x) + \ln^2(x)]$

Further expanding:
$6\ln^3(2) + 5\ln^2(2)\ln(x) + \ln(2)\ln^2(x) + 6\ln^2(2)\ln(x) + 5\ln(2)\ln^2(x) + \ln^3(x)$

Grouping like terms:
$6\ln^3(2) + 11\ln^2(2)\ln(x) + 6\ln(2)\ln^2(x) + \ln^3(x)$

## Step 3: Integrate each term

Now I'll integrate each term of $\frac{\ln(2x)\ln(4x)\ln(8x)}{x}dx$:

1. $\int \frac{6\ln^3(2)}{x}dx = 6\ln^3(2)\ln|x| + C_1$

2. $\int \frac{11\ln^2(2)\ln(x)}{x}dx = 11\ln^2(2)\frac{\ln^2(x)}{2} + C_2 = \frac{11}{2}\ln^2(2)\ln^2(x) + C_2$

3. $\int \frac{6\ln(2)\ln^2(x)}{x}dx = 6\ln(2)\frac{\ln^3(x)}{3} + C_3 = 2\ln(2)\ln^3(x) + C_3$

4. $\int \frac{\ln^3(x)}{x}dx = \frac{\ln^4(x)}{4} + C_4$

Combining these results:
$\int\frac{\ln(2x)\ln(4x)\ln(8x)}{x}dx = 6\ln^3(2)\ln|x| + \frac{11}{2}\ln^2(2)\ln^2(x) + 2\ln(2)\ln^3(x) + \frac{\ln^4(x)}{4} + C$

## Step 4: Evaluate the definite integral

I'll calculate the definite integral by evaluating at the bounds:
$\int_{\frac{1}{8}}^{\frac{1}{4}}\frac{\ln(2x)\ln(4x)\ln(8x)}{x}dx = [6\ln^3(2)\ln|x| + \frac{11}{2}\ln^2(2)\ln^2(x) + 2\ln(2)\ln^3(x) + \frac{\ln^4(x)}{4}]_{\frac{1}{8}}^{\frac{1}{4}}$

For $x = \frac{1}{4}$:
- $\ln(\frac{1}{4}) = \ln(1) - \ln(4) = -\ln(4) = -2\ln(2)$

For $x = \frac{1}{8}$:
- $\ln(\frac{1}{8}) = \ln(1) - \ln(8) = -\ln(8) = -3\ln(2)$

Substituting these values:

At $x = \frac{1}{4}$:
$6\ln^3(2)\ln(\frac{1}{4}) + \frac{11}{2}\ln^2(2)\ln^2(\frac{1}{4}) + 2\ln(2)\ln^3(\frac{1}{4}) + \frac{\ln^4(\frac{1}{4})}{4}$
$= 6\ln^3(2)(-2\ln(2)) + \frac{11}{2}\ln^2(2)(-2\ln(2))^2 + 2\ln(2)(-2\ln(2))^3 + \frac{(-2\ln(2))^4}{4}$
$= -12\ln^4(2) + \frac{11}{2}\ln^2(2) \cdot 4\ln^2(2) + 2\ln(2) \cdot (-8\ln^3(2)) + \frac{16\ln^4(2)}{4}$
$= -12\ln^4(2) + 22\ln^4(2) - 16\ln^4(2) + 4\ln^4(2)$
$= -2\ln^4(2)$

At $x = \frac{1}{8}$:
$6\ln^3(2)\ln(\frac{1}{8}) + \frac{11}{2}\ln^2(2)\ln^2(\frac{1}{8}) + 2\ln(2)\ln^3(\frac{1}{8}) + \frac{\ln^4(\frac{1}{8})}{4}$
$= 6\ln^3(2)(-3\ln(2)) + \frac{11}{2}\ln^2(2)(-3\ln(2))^2 + 2\ln(2)(-3\ln(2))^3 + \frac{(-3\ln(2))^4}{4}$
$= -18\ln^4(2) + \frac{11}{2}\ln^2(2) \cdot 9\ln^2(2) + 2\ln(2) \cdot (-27\ln^3(2)) + \frac{81\ln^4(2)}{4}$
$= -18\ln^4(2) + \frac{99}{2}\ln^4(2) - 54\ln^4(2) + \frac{81}{4}\ln^4(2)$
$= -18\ln^4(2) + 49.5\ln^4(2) - 54\ln^4(2) + 20.25\ln^4(2)$
$= -2.25\ln^4(2)$

Therefore:
$\int_{\frac{1}{8}}^{\frac{1}{4}}\frac{\ln(2x)\ln(4x)\ln(8x)}{x}dx = [-2\ln^4(2)] - [-2.25\ln^4(2)] = 0.25\ln^4(2)$

## Step 5: Numerical approximation

$\ln(2) \approx 0.6931471806$
$\ln^4(2) \approx 0.6931471806^4 \approx 0.2311064613$
$0.25\ln^4(2) \approx 0.25 \times 0.2311064613 \approx 0.0577766153$

Therefore, the definite integral equals $\frac{1}{4}\ln^4(2)$ or approximately $0.0577766153$.

{"answer": "\\frac{1}{4}\\ln^4(2)", "numerical_answer": "0.0577766153"}