# Evaluating $\int_{0}^{1}{\frac{1}{x}}-\left\lfloor{\frac{1}{x}}\right\rfloor\mathrm{d}x$

## Step 1: Understanding the integrand

The integrand is $\frac{1}{x}-\left\lfloor{\frac{1}{x}}\right\rfloor$ where $\left\lfloor{\cdot}\right\rfloor$ represents the floor function.

For $x \in (0,1]$, let's analyze $\frac{1}{x}$ and $\left\lfloor{\frac{1}{x}}\right\rfloor$:

When $x \in (0,1]$, we have $\frac{1}{x} \geq 1$. Specifically:
- For $x \in (\frac{1}{n+1}, \frac{1}{n}]$ where $n$ is a positive integer, we have $\frac{1}{x} \in [n, n+1)$, which means $\left\lfloor{\frac{1}{x}}\right\rfloor = n$.

## Step 2: Break the integral into intervals

Let's split the integral into intervals where the floor function is constant:

$$\int_{0}^{1}\left({\frac{1}{x}}-\left\lfloor{\frac{1}{x}}\right\rfloor\right)\mathrm{d}x = \sum_{n=1}^{\infty}\int_{\frac{1}{n+1}}^{\frac{1}{n}}\left({\frac{1}{x}}-n\right)\mathrm{d}x$$

## Step 3: Compute each piece of the sum

For each $n$, let's compute:
$$\int_{\frac{1}{n+1}}^{\frac{1}{n}}\left({\frac{1}{x}}-n\right)\mathrm{d}x = \left[\ln|x| - nx\right]_{\frac{1}{n+1}}^{\frac{1}{n}}$$

$$= \left(\ln\frac{1}{n} - n \cdot \frac{1}{n}\right) - \left(\ln\frac{1}{n+1} - n \cdot \frac{1}{n+1}\right)$$

$$= -\ln(n) - 1 - (-\ln(n+1) - \frac{n}{n+1})$$

$$= -\ln(n) + \ln(n+1) - 1 + \frac{n}{n+1}$$

$$= \ln\left(\frac{n+1}{n}\right) - 1 + \frac{n}{n+1}$$

$$= \ln\left(1 + \frac{1}{n}\right) - 1 + \frac{n}{n+1}$$

$$= \ln\left(1 + \frac{1}{n}\right) - 1 + \frac{n+1-1}{n+1}$$

$$= \ln\left(1 + \frac{1}{n}\right) - 1 + 1 - \frac{1}{n+1}$$

$$= \ln\left(1 + \frac{1}{n}\right) - \frac{1}{n+1}$$

## Step 4: Sum the series

Now, we need to compute:
$$\sum_{n=1}^{\infty}\left[\ln\left(1 + \frac{1}{n}\right) - \frac{1}{n+1}\right]$$

Let's consider the sum of the logarithms first:
$$\sum_{n=1}^{N}\ln\left(1 + \frac{1}{n}\right) = \sum_{n=1}^{N}\ln\left(\frac{n+1}{n}\right) = \ln\left(\frac{2}{1} \cdot \frac{3}{2} \cdot \frac{4}{3} \cdots \frac{N+1}{N}\right) = \ln(N+1)$$

For the second term:
$$\sum_{n=1}^{N}\frac{1}{n+1} = \sum_{n=2}^{N+1}\frac{1}{n} = \sum_{n=1}^{N+1}\frac{1}{n} - 1 = H_{N+1} - 1$$

Where $H_N$ is the $N$-th harmonic number.

Therefore:
$$\sum_{n=1}^{N}\left[\ln\left(1 + \frac{1}{n}\right) - \frac{1}{n+1}\right] = \ln(N+1) - (H_{N+1} - 1) = \ln(N+1) - H_{N+1} + 1$$

As $N \to \infty$, $\ln(N+1) - H_{N+1}$ approaches the negative of the Euler-Mascheroni constant $-\gamma$. 

Therefore, the sum equals $1-\gamma$.

## Step 5: Final result

$$\int_{0}^{1}\left({\frac{1}{x}}-\left\lfloor{\frac{1}{x}}\right\rfloor\right)\mathrm{d}x = 1-\gamma$$

Where $\gamma \approx 0.5772156649$ is the Euler-Mascheroni constant.

## Numerical approximation
$1-\gamma \approx 1 - 0.5772156649 \approx 0.4227843351$

{"answer": "1-\\gamma", "numerical_answer": "0.4227843351"}