We will show that by a clever change of variable the given integral may be written in closed‐form. In particular, we will prove that

  I = ∫₀² x^(1/2) (2 – x)^(–1/2) cosh(√[x(2 – x)]) dx = π I₀(1),

where I₀(1) is the modified Bessel function of order zero evaluated at 1.

Below are the steps.

Step 1. Make the substitution x = 1 – cosθ.
  When x = 0, we have 1 – cosθ = 0 so cosθ = 1, i.e. θ = 0.
  When x = 2, we have 1 – cosθ = 2 so cosθ = –1, i.e. θ = π.
  Also,
   dx/dθ = sinθ  or  dx = sinθ dθ.
  Now note that
   x^(1/2) = [1 – cosθ]^(1/2)  and  (2 – x)^(–1/2) = [2 – (1 – cosθ)]^(–1/2) = [1 + cosθ]^(–1/2).
  Also, observe that
   √[x(2 – x)] = √[(1 – cosθ)(1 + cosθ)] = √(1 – cos²θ) = sinθ   (since 0 ≤ θ ≤ π, so sinθ ≥ 0).

Thus the integrand becomes
  x^(1/2)(2 – x)^(–1/2) cosh(√[x(2 – x)]) dx
   = [√(1 – cosθ)/√(1 + cosθ)] cosh(sinθ) (sinθ dθ).

Step 2. Simplify the expression.
Recall that the half-angle formula tells us that
  tan(θ/2) = √[(1 – cosθ)/(1 + cosθ)].
Thus,
  [√(1 – cosθ)/√(1 + cosθ)] = tan(θ/2).

Therefore the integral becomes
  I = ∫₀ᵖ tan(θ/2) sinθ cosh(sinθ) dθ.
But note that
  tan(θ/2) = sinθ/(1 + cosθ).
Hence,
  tan(θ/2) sinθ = sin²θ/(1 + cosθ).

Thus, we have
  I = ∫₀^π [sin²θ/(1 + cosθ)] cosh(sinθ) dθ.
Now use the trigonometric identity
  sin²θ = (1 – cosθ)(1 + cosθ).
It follows that
  [sin²θ/(1 + cosθ)] = 1 – cosθ.

Thus the integral reduces to
  I = ∫₀^π [1 – cosθ] cosh(sinθ) dθ
    = ∫₀^π cosh(sinθ) dθ – ∫₀^π cosθ cosh(sinθ) dθ.

Step 3. Show that the second term vanishes.
Consider the second term:
  B = ∫₀^π cosθ cosh(sinθ) dθ.
Make the substitution u = sinθ so that du = cosθ dθ.
When θ = 0, u = 0 and when θ = π, u = sinπ = 0. Hence,
  B = ∫₀⁰ cosh(u) du = 0.
Thus, we are left with
  I = ∫₀^π cosh(sinθ) dθ.

Step 4. Express the remaining integral in closed‐form.
One may now use a standard trick. Write cosh(sinθ) as cos(i sinθ) because cosh(z) = cos(iz). Then we use the known integral formula
  ∫₀^π cos(z sinθ)dθ = π J₀(z),
where J₀(z) is the Bessel function of the first kind of order zero. Taking z = i,
  ∫₀^π cos(i sinθ)dθ = π J₀(i).
But by the standard relation between Bessel functions and modified Bessel functions,
  I₀(1) = J₀(i),
so we deduce that
  I = π I₀(1).

Step 5. Provide a numerical approximation.
It is known that
  I₀(1) ≈ 1.2660658777520082.
Therefore,
  I = π I₀(1) ≈ 3.141592653589793 * 1.2660658777520082 ≈ 3.9782059581.

Thus, the final answer is:

{"answer": "$\\\\pi I_0(1)$", "numerical_answer": "3.9782059581"}