Let's follow each step:

### 1. Compute the integral analytically

We are asked to evaluate:
\[
I = \int_0^\infty \frac{1}{e^x+1} \, dx
\]

### 2. Provide all necessary steps

First, consider a substitution relating this integral to standard integrals.

#### Step 1: Series expansion approach

Notice:
\[
\frac{1}{e^x+1} = \sum_{n=1}^{\infty} (-1)^{n+1} e^{-n x}
\]
This comes from the geometric series expansion:
\[
\frac{1}{1 + y} = \sum_{n=1}^\infty (-1)^{n+1} y^{n-1} \quad \text{for} \ |y| < 1
\]
Set \( y = e^{-x} \), so
\[
\frac{1}{1 + e^{-x}} = \sum_{n=1}^\infty (-1)^{n+1} e^{-(n-1)x}
\]
Apply a shift and for \( \frac{1}{e^{x}+1} \), we get:
\[
\frac{1}{e^{x}+1} = \sum_{n=1}^{\infty} (-1)^{n+1} e^{-n x}
\]
This is valid for \( x > 0 \).

#### Step 2: Integrate term by term

So,
\[
I = \int_0^\infty \frac{1}{e^x+1}\,dx = \int_0^\infty \sum_{n=1}^{\infty} (-1)^{n+1} e^{-n x} dx = \sum_{n=1}^{\infty} (-1)^{n+1} \int_0^\infty e^{-n x} dx
\]
The integral \( \int_0^\infty e^{-n x} dx = \frac{1}{n} \), so:
\[
I = \sum_{n=1}^{\infty} \frac{(-1)^{n+1}}{n}
\]

This is a well-known alternating series:
\[
\sum_{n=1}^{\infty} \frac{(-1)^{n+1}}{n} = \ln(2)
\]

#### **Final analytical answer:**
\[
\boxed{I = \ln 2}
\]

---

### 3. Numerical approximation

\[
\ln 2 \approx 0.6931471806
\]

---

### 4. Final answer in JSON format

```json
{"answer": "\\ln 2", "numerical_answer": "0.6931471806"}
```