<think>
Okay, let's tackle this integral step by step. The problem is to compute the definite integral from 1 to 2 of 2^{x-1} + log base 2 of (2x) dx. Alright, first, I need to break this into two separate integrals because the integral of a sum is the sum of the integrals. So, I can write it as the integral of 2^{x-1} dx plus the integral of log_2(2x) dx, both from 1 to 2.

Starting with the first part: ∫2^{x-1} dx. Hmm, I remember that the integral of a^u is (a^u)/(ln a) + C. So here, the base is 2, and the exponent is x-1. Let me make a substitution. Let u = x - 1, then du = dx. So the integral becomes ∫2^u du, which is (2^u)/(ln 2) + C. Substituting back, that's (2^{x-1})/(ln 2). So evaluated from 1 to 2, that would be [2^{2-1}/(ln 2)] - [2^{1-1}/(ln 2)] = (2^1)/(ln 2) - (2^0)/(ln 2) = (2/ln 2) - (1/ln 2) = (2 - 1)/ln 2 = 1/ln 2. Okay, that's the first part.

Now the second integral: ∫log_2(2x) dx from 1 to 2. Let me simplify the logarithm first. log_2(2x) can be rewritten using logarithm properties. log_b(a*c) = log_b a + log_b c. So log_2(2x) = log_2 2 + log_2 x. Since log_2 2 is 1, this simplifies to 1 + log_2 x. So the integral becomes ∫(1 + log_2 x) dx from 1 to 2. Again, split this into two integrals: ∫1 dx + ∫log_2 x dx.

The first part of that is straightforward: ∫1 dx from 1 to 2 is just [x] from 1 to 2, which is 2 - 1 = 1.

Now the second part: ∫log_2 x dx. To integrate log base 2 of x, I can use integration by parts. Let me recall that ∫log_b x dx = (x log_b x - x)/ln b + C. Alternatively, let's do integration by parts properly. Let u = log_2 x, dv = dx. Then du = (1/(x ln 2)) dx, and v = x. So integration by parts formula is uv - ∫v du. So that's x log_2 x - ∫x*(1/(x ln 2)) dx. Simplify the integral: x log_2 x - ∫(1/ln 2) dx. The integral of 1/ln 2 dx is (1/ln 2)x. So putting it all together: x log_2 x - (x/ln 2) + C.

Therefore, the integral of log_2 x dx is x log_2 x - x/ln 2 + C. So combining the two parts of the second integral: ∫1 dx + ∫log_2 x dx = [x] + [x log_2 x - x/ln 2] evaluated from 1 to 2. Let's compute that.

First, the integral from 1 to 2 of 1 + log_2 x dx is:

At upper limit 2: (2) + (2 log_2 2 - 2/ln 2) = 2 + (2*1 - 2/ln 2) = 2 + 2 - 2/ln 2 = 4 - 2/ln 2.

At lower limit 1: (1) + (1 log_2 1 - 1/ln 2) = 1 + (0 - 1/ln 2) = 1 - 1/ln 2.

Subtracting lower from upper: (4 - 2/ln 2) - (1 - 1/ln 2) = 4 - 2/ln 2 -1 + 1/ln 2 = 3 - (2/ln 2 - 1/ln 2) = 3 - 1/ln 2.

So the second integral evaluates to 3 - 1/ln 2.

Now, combining both integrals: the first integral was 1/ln 2, and the second was 3 - 1/ln 2. So total integral is 1/ln 2 + 3 - 1/ln 2 = 3. Wait, that's interesting. The 1/ln 2 terms cancel out. So the exact answer is 3? Let me check that again.

First integral: 1/ln 2.

Second integral: 3 - 1/ln 2.

Adding them together: 1/ln 2 + 3 - 1/ln 2 = 3. So the exact answer is 3. Hmm, that seems too simple. Let me verify each step.

First integral: ∫1^2 2^{x-1} dx. The antiderivative is 2^{x-1}/ln 2. At x=2: 2^{1}/ln2 = 2/ln2. At x=1: 2^{0}/ln2 = 1/ln2. So difference is (2 -1)/ln2 = 1/ln2. Correct.

Second integral: ∫1^2 log2(2x) dx. We split into 1 + log2 x. Then ∫1 dx is 1. The ∫log2 x dx from 1 to 2 is [x log2 x - x/ln2] from 1 to 2. At x=2: 2*1 - 2/ln2. At x=1: 1*0 -1/ln2. So difference is (2 -2/ln2) - (0 -1/ln2) = 2 -2/ln2 +1/ln2 = 2 -1/ln2. Then adding the 1 from the first part: 1 + (2 -1/ln2) = 3 -1/ln2. Then total integral is 1/ln2 +3 -1/ln2 =3. Yes, that's correct. The terms with ln2 cancel out. So the exact answer is 3. That's surprising but seems right.

Wait, but let me check with numerical approximation. Let's compute the integral numerically to see if it's indeed 3. Let's compute the integral of 2^{x-1} from 1 to 2. The integral of 2^{x-1} is 1/ln2 ≈1.442695041. Then the second integral is 3 -1/ln2 ≈3 -1.442695041≈1.557304959. Adding them gives 1.442695041 +1.557304959=3. So numerically, it's exactly 3. So the exact answer is 3. That's interesting. So the exact answer is 3, and the numerical approximation is 3.0000000000. But wait, is that possible? Let me check with a different approach.

Alternatively, maybe there's a trick here. Let's see. The integrand is 2^{x-1} + log_2(2x). Let me see if this function has an antiderivative that can be simplified. Let's check the derivative of 2^{x}/ln2. The derivative is 2^{x} ln2 / ln2 =2^{x}. But our first term is 2^{x-1} = (1/2)2^{x}. So the antiderivative of 2^{x-1} is (1/2)(2^{x}/ln2) )= 2^{x-1}/ln2, which matches what we had before.

For the second part, log_2(2x) =1 + log2 x. The integral of 1 is x. The integral of log2 x is x log2 x -x /ln2. So when we combine all terms, the antiderivative is 2^{x-1}/ln2 + x +x log2 x -x/ln2. Then when we evaluate from 1 to 2.

At x=2: 2^{1}/ln2 +2 +2*1 -2/ln2 = (2/ln2) +2 +2 -2/ln2 = (2/ln2 -2/ln2) +4=4.

At x=1: 2^{0}/ln2 +1 +1*0 -1/ln2 = (1/ln2) +1 -1/ln2=1.

So the difference is 4 -1=3. So that's correct. Therefore, the exact answer is 3, and the numerical approximation is exactly 3.0000000000. So the answer is 3. So the JSON should be {"answer": "3", "numerical_answer": "3.0000000000"}.
</think>

{"answer": "3", "numerical_answer": "3.0000000000"}