We wish to evaluate

  I = ∫₀² x^(–1/2) (1 + √(x(2 – x)))^(–3/2) dx.

A very effective way to attack this integral is to use a substitution that “absorbs” the square roots. We shall describe one route that leads to an answer in closed form.

Step 1. Let
  x = 2 sin²θ.
Then when x = 0, θ = 0, and when x = 2, θ = π/2. Also,
  dx/dθ = 4 sinθ cosθ ⟹ dx = 4 sinθ cosθ dθ.
Moreover,
  x^(–1/2) = (2 sin²θ)^(–1/2) = 1/(√2 sinθ),
and note that
  x(2 – x) = 2 sin²θ (2 – 2 sin²θ) = 4 sin²θ cos²θ ⟹ √(x(2 – x)) = 2 sinθ cosθ.

Thus the integrand becomes:
  x^(–1/2)(1 + √(x(2 – x)))^(–3/2) dx
    = [1/(√2 sinθ)] · [1 + 2 sinθ cosθ]^(–3/2) · (4 sinθ cosθ dθ)
    = [4 cosθ/(√2)] · [1 + 2 sinθ cosθ]^(–3/2) dθ
    = 2√2 cosθ (1 + sin2θ)^(–3/2) dθ            [since sin2θ = 2 sinθ cosθ].

So the integral becomes:
  I = 2√2 ∫₀^(π/2) cosθ (1 + sin2θ)^(–3/2) dθ.

Step 2. To simplify further, shift the variable via a cosine double–angle identity. Set
  θ = z + π/4.
Then when θ goes from 0 to π/2, z runs from –π/4 to π/4. Note that:
  sin2θ = sin(2z + π/2) = cos2z,
and
  cosθ = cos(z + π/4) = (cosz – sinz)/√2.

Therefore,
  I = 2√2 ∫_(z=–π/4)^(π/4) [ (cosz – sinz)/√2 ] (1 + cos2z)^(–3/2) dz
    = 2 ∫_(–π/4)^(π/4) (cosz – sinz) (1 + cos2z)^(–3/2) dz.

Recall that a standard trigonometric identity gives:
  1 + cos2z = 2 cos²z.
Thus,
  (1 + cos2z)^(–3/2) = (2 cos²z)^(–3/2) = 2^(–3/2) cos^(–3)z.

So now the integral becomes:
  I = 2 · 2^(–3/2) ∫_(–π/4)^(π/4) (cosz – sinz) cos^(–3)z dz
    = (2^(1–3/2)) ∫_(–π/4)^(π/4) (cosz – sinz) sec³z dz
    = (1/√2) ∫_(–π/4)^(π/4) (cosz – sinz) sec³z dz.

Write sec³z = sec²z · sec z and combine with cosz – sinz:
  (cosz – sinz) sec³z = (cosz sec³z) – (sinz sec³z)
    = sec²z – tanz sec²z       [since cosz·sec³z = sec²z and sinz·sec³z = tanz sec²z].
Thus,
  I = (1/√2) ∫_(–π/4)^(π/4) sec²z (1 – tanz) dz.

Step 3. Make the substitution u = tanz. Then
  du/dz = sec²z, or du = sec²z dz.
When z = –π/4, u = tan(–π/4) = –1, and when z = π/4, u = tan(π/4) = 1.
Therefore, the integral becomes:
  I = (1/√2) ∫_(u=–1)^(1) (1 – u) du.

Step 4. Evaluate the u–integral:
  ∫_(–1)^(1) (1 – u) du = [u – (u²)/2]_(–1)^(1).
Compute at u = 1:
  1 – 1/2 = 1/2.
At u = –1:
  (–1) – (1/2) = –3/2.
Thus, the difference is:
  (1/2) – (–3/2) = 2.
So,
  I = (1/√2) · 2 = (2/√2) = √2.

Step 5. Conclude the result

The exact answer is:
  I = √2.

The corresponding numerical value (to 10 decimal places) is approximately 1.4142135624.

Finally, we output the answer in the required JSON format:

{"answer": "\\sqrt{2}", "numerical_answer": "1.4142135624"}