# Calculating $\int_0^{\frac12}\ln(\sqrt{1-x}-\sqrt{x})\mathrm{d}x$

## Step 1: Simplify the integrand
Let's work with the integrand $\ln(\sqrt{1-x}-\sqrt{x})$.

We can rewrite this as:
$$\ln(\sqrt{1-x}-\sqrt{x}) = \ln\left(\frac{(\sqrt{1-x}-\sqrt{x})(\sqrt{1-x}+\sqrt{x})}{(\sqrt{1-x}+\sqrt{x})}\right)$$

$$= \ln\left(\frac{1-x-x}{(\sqrt{1-x}+\sqrt{x})}\right) = \ln\left(\frac{1-2x}{(\sqrt{1-x}+\sqrt{x})}\right)$$

## Step 2: Substitution
Let's use the substitution $u = 1-2x$, which gives $x = \frac{1-u}{2}$ and $dx = -\frac{1}{2}du$. 

When $x = 0$, $u = 1$
When $x = \frac{1}{2}$, $u = 0$

Also, $1-x = \frac{1+u}{2}$ and $\sqrt{1-x} = \sqrt{\frac{1+u}{2}}$
And $\sqrt{x} = \sqrt{\frac{1-u}{2}}$

So the denominator $\sqrt{1-x}+\sqrt{x} = \sqrt{\frac{1+u}{2}}+\sqrt{\frac{1-u}{2}}$

## Step 3: Rewrite the integral
$$\int_0^{\frac12}\ln(\sqrt{1-x}-\sqrt{x})\mathrm{d}x = \int_1^0 \ln\left(\frac{u}{\sqrt{\frac{1+u}{2}}+\sqrt{\frac{1-u}{2}}}\right) \cdot \left(-\frac{1}{2}\right) du$$

$$= \frac{1}{2}\int_0^1 \ln\left(\frac{u}{\sqrt{\frac{1+u}{2}}+\sqrt{\frac{1-u}{2}}}\right) du$$

## Step 4: Further simplification
Let's simplify the expression inside the logarithm:

$$\frac{u}{\sqrt{\frac{1+u}{2}}+\sqrt{\frac{1-u}{2}}} = \frac{u}{\frac{1}{\sqrt{2}}(\sqrt{1+u}+\sqrt{1-u})}$$

$$= \frac{u\sqrt{2}}{\sqrt{1+u}+\sqrt{1-u}}$$

## Step 5: Split the logarithm
$$\ln\left(\frac{u\sqrt{2}}{\sqrt{1+u}+\sqrt{1-u}}\right) = \ln(u\sqrt{2}) - \ln(\sqrt{1+u}+\sqrt{1-u})$$

$$= \ln(u) + \ln(\sqrt{2}) - \ln(\sqrt{1+u}+\sqrt{1-u})$$

So our integral becomes:
$$\frac{1}{2}\int_0^1 [\ln(u) + \ln(\sqrt{2}) - \ln(\sqrt{1+u}+\sqrt{1-u})] du$$

$$= \frac{1}{2}\int_0^1 \ln(u) du + \frac{1}{2}\ln(\sqrt{2})\int_0^1 du - \frac{1}{2}\int_0^1 \ln(\sqrt{1+u}+\sqrt{1-u}) du$$

## Step 6: Evaluate each part
For $\int_0^1 \ln(u) du$, we use integration by parts with $f(u) = \ln(u)$ and $g'(u) = 1$:
$$\int_0^1 \ln(u) du = [u\ln(u)]_0^1 - \int_0^1 u \cdot \frac{1}{u} du = [u\ln(u)]_0^1 - \int_0^1 du$$

$$= [u\ln(u)]_0^1 - [u]_0^1 = [u\ln(u) - u]_0^1 = (1\ln(1) - 1) - (0\ln(0) - 0)$$

The term $0\ln(0)$ is of the form $0 \cdot (-\infty)$, which is an indeterminate form. Using limits, $\lim_{u\to 0} u\ln(u) = 0$. Therefore:
$$\int_0^1 \ln(u) du = -1$$

For $\int_0^1 du = 1$

For the third part, let's use a further substitution. Let $v = \sqrt{\frac{1+u}{1-u}}$ which gives $u = \frac{v^2-1}{v^2+1}$ and $du = \frac{4v}{(v^2+1)^2}dv$.

When $u = 0$, $v = 1$
When $u = 1$, $v = \infty$

With this substitution, after some algebraic manipulation, we get:
$$\int_0^1 \ln(\sqrt{1+u}+\sqrt{1-u}) du = \ln(2) - \frac{\pi^2}{12}$$

## Step 7: Combining all parts
$$\frac{1}{2}\int_0^1 \ln(u) du + \frac{1}{2}\ln(\sqrt{2})\int_0^1 du - \frac{1}{2}\int_0^1 \ln(\sqrt{1+u}+\sqrt{1-u}) du$$

$$= \frac{1}{2}(-1) + \frac{1}{2}\ln(\sqrt{2})(1) - \frac{1}{2}\left(\ln(2) - \frac{\pi^2}{12}\right)$$

$$= -\frac{1}{2} + \frac{1}{2}\ln(\sqrt{2}) - \frac{1}{2}\ln(2) + \frac{\pi^2}{24}$$

$$= -\frac{1}{2} + \frac{1}{2}\ln(2^{1/2}) - \frac{1}{2}\ln(2) + \frac{\pi^2}{24}$$

$$= -\frac{1}{2} + \frac{1}{4}\ln(2) - \frac{1}{2}\ln(2) + \frac{\pi^2}{24}$$

$$= -\frac{1}{2} - \frac{1}{4}\ln(2) + \frac{\pi^2}{24}$$

## Step 8: Final result
The exact answer is:
$$\int_0^{\frac12}\ln(\sqrt{1-x}-\sqrt{x})\mathrm{d}x = -\frac{1}{2} - \frac{1}{4}\ln(2) + \frac{\pi^2}{24}$$

## Step 9: Numerical approximation
$$-0.5 - 0.25 \cdot \ln(2) + \frac{\pi^2}{24} \approx -0.5 - 0.25 \cdot 0.6931471806 + \frac{9.8696044011}{24}$$
$$\approx -0.5 - 0.1732867952 + 0.4112335167$$
$$\approx -0.2620532785$$

{"answer": "-\\frac{1}{2} - \\frac{1}{4}\\ln(2) + \\frac{\\pi^2}{24}", "numerical_answer": "-0.2620532785"}