Let's denote the integral:
\[
I = \int_{0}^{1} \frac{1}{\sqrt{1+x}} \ln\left(\sqrt{x} + \sqrt{1+x}\right) \, \mathrm{E}(\sqrt{1-x}) \, dx
\]
where \(\mathrm{E}(k)\) is the complete elliptic integral of the second kind.

Let's follow the steps as requested:

---

**Step 1 & 2: Analytic Computation**

We will first try to simplify the integrand.

Let us note:

- The complete elliptic integral of the second kind is:
  \[
  \mathrm{E}(k) = \int_0^{\pi/2} \sqrt{1 - k^2 \sin^2 \theta} \, d\theta
  \]
  For our integrand, the argument is \(k = \sqrt{1-x}\).

- The logarithmic term:
  \[
  \ln\left(\sqrt{x} + \sqrt{1+x}\right)
  \]

Let us attempt a substitution to simplify the logarithmic and square root expressions.

Let us try \(x = \sinh^2 t\), so \(dx = 2\sinh t \cosh t dt\), \(x \in [0,1]\) implies \(t \in [0,\operatorname{arcsinh}(1)]\).

- \(\sqrt{1+x} = \sqrt{1 + \sinh^2 t} = \sqrt{\cosh^2 t} = \cosh t\)
- \(\sqrt{x} = \sinh t\)
- \(\ln(\sqrt{x} + \sqrt{1+x}) = \ln(\sinh t + \cosh t) = \ln(e^t) = t\)

So, \(\ln(\sqrt{x} + \sqrt{1+x}) = t\).

- \(\sqrt{1-x} = \sqrt{1 - \sinh^2 t} = \sqrt{\cosh^2 t - \sinh^2 t} = \sqrt{1} = 1\). Wait: but \(1-\sinh^2 t = \cosh^2 t - \sinh^2 t = 1\), which is always 1. That can't be: for \(x=1, t = \operatorname{arcsinh}(1)\), so...

Wait: \(\sinh^2 t\) from \(t=0\) to \(t_1 = \operatorname{arcsinh}(1)\), that's from \(x=0\) to \(x=1\).

But \(\sqrt{1-x} = \sqrt{1-\sinh^2 t}\).

But \(\cosh^2 t - \sinh^2 t = 1\) â‡’ \(\cosh^2 t = 1 + \sinh^2 t\), so \(1 - \sinh^2 t = \cosh^2 t - \sinh^2 t = 1\), always 1. So \(\sqrt{1-x} = 1\) always in this variable, which is an unexpected simplification.

Therefore, after this substitution:

- \(\frac{1}{\sqrt{1 + x}} = \frac{1}{\cosh t}\)
- \(dx = 2 \sinh t \cosh t dt\)
- \(\ln(\sqrt{x} + \sqrt{1+x}) = t\)
- \(\operatorname{E}(\sqrt{1-x}) = \operatorname{E}(1)\), which is the complete elliptic integral of the second kind at \(k=1\).

But \(\operatorname{E}(1) = 1\), but this is *not* correct: the value is \(\operatorname{E}(1) = 1\) only for the integral on [0, pi/2], but in fact, \(\operatorname{E}(1) = \int_0^{\pi/2} \sqrt{1-\sin^2\theta}d\theta = \int_0^{\pi/2} \cos \theta d\theta = 1\).

Yes, so \(\operatorname{E}(1) = 1\).

So the whole integrand, after substitution, is:
\[
\frac{1}{\cosh t} \cdot t \cdot 1 \cdot 2 \sinh t \cosh t \, dt = 2 t \sinh t \, dt
\]

The bounds are \(t=0\) (\(x=0\)), \(t_1 = \operatorname{arcsinh}(1)\) (\(x=1\)):
- \(t_1 = \ln(1 + \sqrt{1+1^2}) = \ln(1 + \sqrt{2}) \approx 0.8813735870\)

So the integral reduces to:
\[
I = 2 \int_{t=0}^{t=\ln(1+\sqrt{2})} t \sinh t \, dt
\]

Let's compute this elementary integral:

Recall:
\[
\int t \sinh t \, dt = t \cosh t - \int \cosh t \, dt = t\cosh t - \sinh t + C
\]

Therefore,
\[
I = 2 \left[ t \cosh t - \sinh t \right]_{0}^{\ln(1+\sqrt{2})}
\]

Thus,
\[
I = 2 \left \{ \left[ t_1 \cosh t_1 - \sinh t_1 \right] - [ 0 \cdot \cosh 0 - \sinh 0 ] \right\}
\]

But at \(t=0\), \(\cosh(0) = 1\), \(\sinh(0)=0\), so the lower bound is 0.

Therefore,
\[
I = 2 \left[ t_1 \cosh t_1 - \sinh t_1 \right]
\]

where \(t_1 = \ln(1+\sqrt{2})\).

Let's compute \(\cosh t_1\) and \(\sinh t_1\).

Let \(A = \ln(1+\sqrt{2})\).

Recall:
\[
\cosh A = \frac{e^A + e^{-A}}{2}, \qquad \sinh A = \frac{e^A - e^{-A}}{2}
\]

But \(e^A = 1+\sqrt{2}\), so \(e^{-A} = 1/(1+\sqrt{2})\).

Thus,
\[
\cosh A = \frac{1+\sqrt{2} + \frac{1}{1+\sqrt{2}}}{2},\qquad
\sinh A = \frac{1+\sqrt{2} - \frac{1}{1+\sqrt{2}}}{2}
\]

But \(1+\sqrt{2} \approx 2.414213562\), so its reciprocal is \(1/(1+\sqrt{2}) \approx 0.4142135624\).

So
\[
\cosh A \approx \frac{2.414213562 + 0.4142135624}{2} = \frac{2.828427124}{2} = 1.414213562
\]
\[
\sinh A \approx \frac{2.414213562 - 0.4142135624}{2} = \frac{2.0}{2} = 1.0
\]

Now assemble:
\[
I = 2 \left[ A \cosh A - \sinh A \right]
\]

Plugging the numbers:
\[
A = \ln(1+\sqrt{2}) \approx 0.8813735870 \\
\cosh A \approx 1.414213562 \\
\sinh A = 1.0
\]
\[
A \cosh A = 0.8813735870 \times 1.414213562 \approx 1.247418379
\]
\[
I = 2 [1.247418379 - 1.0] = 2 \times 0.247418379 = 0.4948367582
\]

---

**Step 3: Numerical approximation (rounded to 10 decimal places)**

Numerical answer: \(0.4948367582\)

---

**Step 4: Final answer in JSON format**

```json
{"answer": "2 \\left[ \\ln(1+\\sqrt{2}) \\cdot \\cosh(\\ln(1+\\sqrt{2})) - \\sinh(\\ln(1+\\sqrt{2})) \\right]", "numerical_answer": "0.4948367582"}
```
