Given the integral:
\[
I = \int_0^1 x^{-1/4} (1-x)^{1/4} I_1\left( \sqrt[4]{x(1-x)} \right) dx
\]
where \( I_1 \) is the modified Bessel function of the first kind.

Let's proceed step by step.

---

### Step 1: Series representation for \( I_1(z) \)

The modified Bessel function of the first kind has the series expansion:
\[
I_1(z) = \sum_{k=0}^{\infty} \frac{1}{k! \Gamma(k+2)} \left( \frac{z}{2} \right)^{2k+1}
\]

Let's set \( z = \sqrt[4]{x(1-x)} \):

\[
I_1\left(\sqrt[4]{x(1-x)}\right) = \sum_{k=0}^{\infty} \frac{1}{k! \Gamma(k+2)} \frac{\left(x(1-x)\right)^{(2k+1)/4}}{2^{2k+1}}
\]

---

### Step 2: Substitute series into the integral

Insert this into the integral:

\[
I = \int_0^1 x^{-1/4} (1-x)^{1/4} \sum_{k=0}^{\infty} \frac{1}{k! \Gamma(k+2)} \frac{\left(x(1-x)\right)^{(2k+1)/4}}{2^{2k+1}} dx
\]

Interchange sum and integral (justified by uniform convergence over compact interval and nonnegative terms):

\[
I = \sum_{k=0}^{\infty} \frac{1}{k! \Gamma(k+2) 2^{2k+1}} \int_0^1 x^{-1/4} (1-x)^{1/4} \left(x(1-x)\right)^{(2k+1)/4} dx
\]

---

### Step 3: Combine exponents and simplify the integral

\[
x^{-1/4} \cdot x^{(2k+1)/4} = x^{(2k+1)/4 - 1/4} = x^{2k/4} = x^{k/2}
\]
and
\[
(1-x)^{1/4} \cdot (1-x)^{(2k+1)/4} = (1-x)^{(2k+1+1)/4} = (1-x)^{(2k+2)/4} = (1-x)^{(k+1)/2}
\]

So,
\[
\int_0^1 x^{-1/4} (1-x)^{1/4} \left(x(1-x)\right)^{(2k+1)/4} dx = \int_0^1 x^{k/2} (1-x)^{(k+1)/2} dx
\]

---

### Step 4: Identify as Beta integral

The Beta function is:
\[
B(a,b) = \int_0^1 x^{a-1}(1-x)^{b-1} dx = \frac{\Gamma(a)\Gamma(b)}{\Gamma(a+b)}
\]

So,
\[
x^{k/2} = x^{(k/2)}, \quad (1-x)^{(k+1)/2} = (1-x)^{(k+1)/2}
\]
So, comparing to Beta, requires:
\[
a-1 = k/2 \implies a = k/2 + 1
\]
\[
b-1 = (k+1)/2 \implies b = (k+1)/2 + 1 = (k+3)/2
\]

Therefore,
\[
\int_0^1 x^{k/2} (1-x)^{(k+1)/2} dx = B\left(\frac{k}{2}+1, \frac{k+3}{2}\right)
\]

---

### Step 5: Substitute everything back

Now:
\[
I = \sum_{k=0}^{\infty} \frac{1}{k! \Gamma(k+2) 2^{2k+1}} B\left(\frac{k}{2} + 1, \frac{k+3}{2}\right)
\]

But recall that:
\[
B(a,b) = \frac{\Gamma(a)\Gamma(b)}{\Gamma(a+b)}
\]

So,
\[
I = \sum_{k=0}^{\infty} \frac{1}{k! \Gamma(k+2) 2^{2k+1}} \cdot \frac{\Gamma\left(\frac{k}{2}+1\right) \Gamma\left(\frac{k+3}{2}\right)}{\Gamma(k+2)}
\]

That is,
\[
\boxed{
I = \sum_{k=0}^{\infty} \frac{\Gamma\left(\frac{k}{2}+1\right) \Gamma\left(\frac{k+3}{2}\right)}{k! \left[\Gamma(k+2)\right]^2 2^{2k+1}}
}
\]

---

### Step 6: Try to further simplify

Let's check if we can further reduce the Gamma expressions.

- \(\Gamma(k+2) = (k+1)!\)
- But the rest are less obvious.

So the closed-form expression is as above.

---

### Step 7: Numerical evaluation

Let's compute the sum for \(k\) up to, say, 10, and check convergence.

Letâ€™s evaluate the first few terms:

#### For \( k = 0 \):
\[
\Gamma\left(\frac{0}{2}+1\right) = \Gamma(1) = 1
\]
\[
\Gamma\left(\frac{0+3}{2}\right) = \Gamma(1.5) = \frac{\sqrt{\pi}}{2}
\]
\[
k! = 1
\]
\[
\Gamma(0+2) = \Gamma(2) = 1!
\]
So
\[
I_0 = \frac{1 \cdot \frac{\sqrt{\pi}}{2}}{1 \cdot 1 \cdot 2^{1}} = \frac{\sqrt{\pi}}{4}
\]
Value: \(\sqrt{\pi}/4 \approx 0.4431134627\)

---

#### For \( k = 1 \):

\[
\Gamma(1/2+1) = \Gamma(1.5) = \frac{\sqrt{\pi}}{2}
\]
\[
\Gamma((1+3)/2) = \Gamma(2) = 1
\]
\[
1! = 1
\]
\[
\Gamma(1+2) = \Gamma(3) = 2!
\]
So
\[
I_1 = \frac{\left(\frac{\sqrt{\pi}}{2}\right) \cdot 1}{1 \cdot 2^2 \cdot 2^2} = \frac{\frac{\sqrt{\pi}}{2}}{1 \cdot 4 \cdot 4} = \frac{\sqrt{\pi}}{32}
\]
But be careful:

Numerator: \(\frac{\sqrt{\pi}}{2}\)

Denominator: \(1 \cdot (2!)^2 \cdot 2^{3}\)

Wait! The formula is:

\[
I_1 = \frac{\Gamma(1.5) \Gamma(2)}{1! [\Gamma(3)]^2 2^{3}} = \frac{\frac{\sqrt{\pi}}{2} \cdot 1}{1 \cdot (2)^2 \cdot 8} = \frac{\frac{\sqrt{\pi}}{2}}{4 \cdot 8} = \frac{\sqrt{\pi}}{64}
\]
But this doesn't match the full expression. Let's double-check the denominator.

For \(k=1\):

- \(k! = 1\)
- \(\Gamma(k+2) = \Gamma(3) = 2!\), squared is \(4\).
- \(2^{2k+1} = 2^{3} = 8\).

So total denominator is \(1 \cdot 4 \cdot 8 = 32\).

So
\[
I_1 = \frac{\frac{\sqrt{\pi}}{2} \times 1}{32} = \frac{\sqrt{\pi}}{64}
\]

Value: \(\sqrt{\pi}/64 \approx 0.02769459142\)

---

#### For \( k = 2 \):

\[
\Gamma(2) = 1!
\]
\[
\Gamma(2.5) = \frac{3}{4} \sqrt{\pi}
\]
\[
2! = 2
\]
\[
\Gamma(4) = 3! = 6
\]
\[
2^{5} = 32
\]
So the denominator: \(2 \cdot 36 \cdot 32 = 2304\)

Numerator: \(1 \cdot \frac{3}{4} \sqrt{\pi} = \frac{3}{4} \sqrt{\pi}\)

So
\[
I_2 = \frac{\frac{3}{4} \sqrt{\pi}}{2304} = \frac{3 \sqrt{\pi}}{9216}
\]

\(\sqrt{\pi} \approx 1.77245\), so
\[
\frac{3 \cdot 1.77245}{9216} \approx \frac{5.31735}{9216} \approx 0.00057659808
\]

---

#### For \( k = 3 \):

\[
\Gamma(2.5) = \frac{3}{4} \sqrt{\pi}
\]
\[
\Gamma(3) = 2!
\]
\[
3! = 6
\]
\[
\Gamma(5) = 4! = 24
\]
\[
2^{7} = 128
\]

\[
\text{Numerator: } \frac{3}{4} \sqrt{\pi} \cdot 2 = \frac{3}{2} \sqrt{\pi}
\]
\[
\text{Denominator: } 6 \cdot 24^2 \cdot 128 = 6 \cdot 576 \cdot 128 = 6 \cdot 73728 = 442368
\]
So
\[
I_3 = \frac{3 \sqrt{\pi}}{2 \cdot 442368} = \frac{3 \sqrt{\pi}}{884736}
\]
Value: \(3 \cdot 1.77245 = 5.31735\), \(5.31735/884736 \approx 0.0000060110\)

---

#### Quickly sum these four terms:
\[
0.4431134627 + 0.02769459142 + 0.00057659808 + 0.0000060110 \approx 0.4713906632
\]

Higher terms become rapidly negligible. Let's check with one more:

#### For \( k = 4 \):

\[
\Gamma(3) = 2!
\]
\[
\Gamma(3.5) = \frac{3}{4} \cdot \frac{5}{2} \sqrt{\pi} = \frac{15}{8}\sqrt{\pi}
\]
\[
4! = 24
\]
\[
\Gamma(6) = 5! = 120
\]
\[
2^9 = 512
\]

\[
\text{Numerator: } 2 \cdot \frac{15}{8}\sqrt{\pi} = \frac{15}{4}\sqrt{\pi}
\]
\[
\text{Denominator: } 24 \cdot (120)^2 \cdot 512 = 24 \cdot 14400 \cdot 512 = 24 \cdot 7372800 = 176947200
\]

\[
I_4 = \frac{15 \sqrt{\pi}}{4 \cdot 176947200} = \frac{15 \sqrt{\pi}}{707788800}
\]
Value: \(15 \cdot 1.77245 \approx 26.58675\), so
\(26.58675 / 707788800 \approx 0.00000003756\)

This term is negligible.

---

Sum so far: \(0.4431134627 + 0.02769459142 + 0.00057659808 + 0.0000060110 \approx 0.4713906632\)

So rounded to 10 digits, \(I \approx 0.4713906632\).

---

## Final JSON answer

```json
{"answer": "\\sum_{k=0}^{\\infty} \\frac{\\Gamma\\left(\\frac{k}{2}+1\\right) \\Gamma\\left(\\frac{k+3}{2}\\right)}{k! [\\Gamma(k+2)]^2 2^{2k+1}}", "numerical_answer": "0.4713906632"}
```