<think>
Okay, let's tackle this integral step by step. The integral is ∫₀¹ (x³ + x + 1)/(3x² - 3x + 4) dx. Hmm, first, I need to simplify the integrand. The denominator is a quadratic, so maybe polynomial long division would help here since the numerator is a cubic. Let me check the degrees: numerator is degree 3, denominator is degree 2. So, the division should give a linear term plus a remainder over the denominator.

Let me set it up. Divide x³ + x + 1 by 3x² - 3x + 4. Let's see, the leading term of the numerator is x³, and the denominator's leading term is 3x². So, the first term in the quotient is (x³)/(3x²) = x/3. Multiply the denominator by x/3: (3x² - 3x + 4)*(x/3) = x³ - x² + (4/3)x. Subtract that from the original numerator:

(x³ + x + 1) - (x³ - x² + (4/3)x) = 0x³ + x² - (1/3)x + 1.

Now, the new numerator is x² - (1/3)x + 1. The denominator is still 3x² - 3x + 4. The degree of the remainder (2) is equal to the degree of the denominator (2), so we can continue the division. The next term is (x²)/(3x²) = 1/3. Multiply the denominator by 1/3: (3x² - 3x + 4)*(1/3) = x² - x + 4/3. Subtract that from the current remainder:

(x² - (1/3)x + 1) - (x² - x + 4/3) = [0x²] + (2/3)x - 1/3.

So now, the integral becomes the integral of the quotient (x/3 + 1/3) plus the remainder ( (2/3)x - 1/3 ) divided by the denominator (3x² - 3x + 4). So:

Integral = ∫ (x/3 + 1/3) dx + ∫ [(2/3)x - 1/3]/(3x² - 3x + 4) dx.

Let me split this into two parts. The first integral is straightforward. Let's compute that first part:

∫ (x/3 + 1/3) dx from 0 to 1. Integrate term by term:

(1/3)*(x²/2) + (1/3)x evaluated from 0 to 1. That gives (1/6)x² + (1/3)x from 0 to 1. Plugging in 1: (1/6)(1) + (1/3)(1) = 1/6 + 1/3 = 1/6 + 2/6 = 3/6 = 1/2. At 0, it's 0. So the first part is 1/2.

Now, the second integral: ∫ [(2/3)x - 1/3]/(3x² - 3x + 4) dx from 0 to 1. Let's simplify the denominator. Let me denote the denominator as D = 3x² - 3x + 4. Let's compute its derivative: D' = 6x - 3. Hmm, the numerator is (2/3)x - 1/3. Let's see if we can express the numerator as a multiple of D' plus a constant.

Let me write (2/3)x - 1/3 = A*(6x - 3) + B. Let's solve for A and B.

Expanding the right side: 6A x - 3A + B. Comparing coefficients:

6A = 2/3 ⇒ A = (2/3)/6 = 1/9.

Then, the constant term: -3A + B = -1/3. Plugging A = 1/9:

-3*(1/9) + B = -1/3 ⇒ -1/3 + B = -1/3 ⇒ B = 0.

So, (2/3)x - 1/3 = (1/9)(6x - 3). Therefore, the integral becomes:

∫ (1/9)(6x - 3)/(3x² - 3x + 4) dx.

This is (1/9) ∫ (6x - 3)/D dx, where D = 3x² - 3x + 4. Notice that the numerator is exactly the derivative of D. Because D' = 6x - 3. So, this integral is (1/9) ∫ D'/D dx = (1/9) ln|D| + C. So, the integral from 0 to 1 is (1/9)[ln|D|] from 0 to 1.

But we also need to check if there's a remaining term. Wait, since we expressed the entire numerator as (1/9)(6x - 3), which is D', then the integral is straightforward. So, the second part is (1/9) [ln|3x² - 3x +4|] from 0 to 1.

Wait, but let me check again. The original integral after division was:

∫ (x/3 + 1/3) dx + ∫ [(2/3)x -1/3]/D dx. Then, we expressed the second integral as (1/9) ∫ D'/D dx. So yes, that's correct. Therefore, the second integral is (1/9) [ln(D)] from 0 to 1.

So, combining both parts, the total integral is:

[1/2] + (1/9)[ln(3(1)^2 -3(1) +4) - ln(3(0)^2 -3(0) +4)].

Compute the values inside the logarithms:

At x=1: 3(1) -3(1) +4 = 3 -3 +4 =4.

At x=0: 0 -0 +4=4.

So, ln(4) - ln(4) =0. Wait, that can't be right. That would make the second integral zero, but that's not possible. Wait, but according to the calculation, the second integral is (1/9)(ln(4) - ln(4))=0. But that would mean the entire integral is 1/2 +0=1/2. But that seems too simple. Let me check my steps again.

Wait, perhaps I made a mistake in the polynomial division. Let me verify that.

Original numerator: x³ +x +1. Divided by 3x² -3x +4.

First term: x³ /3x² = x/3. Multiply divisor by x/3: (3x² -3x +4)(x/3) = x³ -x² + (4/3)x. Subtract from numerator:

(x³ +x +1) - (x³ -x² + (4/3)x) = 0x³ +x² - (1/3)x +1. Correct.

Next term: x² /3x² =1/3. Multiply divisor by 1/3: (3x² -3x +4)(1/3)=x² -x +4/3. Subtract:

(x² - (1/3)x +1) - (x² -x +4/3) = [0x²] + (2/3)x -1/3. Correct.

So the division is correct.

Then, the integral becomes (x/3 +1/3) + (2/3x -1/3)/D. Then, when we split the integral, the first part is 1/2. The second part is ∫ (2/3x -1/3)/D dx. Then, we set (2/3x -1/3) = A*(6x -3) + B. Solving gives A=1/9, B=0. So, the integral is (1/9)∫D’/D dx = (1/9)ln|D|. Evaluated from 0 to1, which gives (1/9)(ln4 - ln4)=0. So the total integral is 1/2. But that seems counterintuitive. How can the integral of a positive function over [0,1] be exactly 1/2? Let me check with a numerical approximation.

Alternatively, maybe there's a mistake in the setup. Let me compute the integral numerically to check.

Wait, but let's compute the integral of (x³ +x +1)/(3x² -3x +4) from 0 to1. Let me plug in x=0: (0 +0 +1)/(0 -0 +4)=1/4. At x=1: (1 +1 +1)/(3 -3 +4)=3/4. The function starts at 1/4 and ends at 3/4. The integral is 1/2? That seems possible if the function is symmetric or something. But maybe it's correct. Let me compute a rough numerical estimate. For example, using trapezoidal rule with two intervals: at x=0, 0.25; x=0.5, and x=1.

At x=0: 1/4=0.25.

At x=0.5: (0.125 +0.5 +1)/(3*(0.25) -3*(0.5) +4) = (1.625)/(0.75 -1.5 +4)=1.625/3.25=0.5.

At x=1: 3/4=0.75.

Trapezoidal rule: (0.5 -0)/2 * [0.25 + 2*0.5 +0.75] = 0.25*(0.25 +1 +0.75)=0.25*(2)=0.5. So the trapezoidal estimate with two intervals gives 0.5. So maybe the exact answer is indeed 1/2. But that's surprising. So according to the analytical solution, the integral is 1/2. But let me check again.

Wait, but according to the steps, the integral is 1/2 +0=1/2. But the numerical approximation also gives 0.5. So maybe it's correct. But why does the second integral evaluate to zero? Because the denominator at x=1 and x=0 is 4, so ln(4)-ln(4)=0. So the second part is zero. So the total integral is 1/2. That's interesting. So the exact answer is 1/2, and the numerical approximation is 0.5. So the answer is 1/2. But let me check with another method.

Alternatively, maybe there's a substitution that can be done. Let me consider the denominator 3x² -3x +4. Let me complete the square. 3x² -3x +4 =3(x² -x) +4=3(x² -x +1/4) +4 -3*(1/4)=3(x -1/2)^2 +4 -3/4=3(x -1/2)^2 +13/4. So the denominator is always positive, which is good.

But perhaps another approach. Let me see if the original integrand can be expressed as derivative of denominator plus something. But maybe not necessary here. According to the previous steps, the integral is 1/2. Let me check with another numerical method. For example, Simpson's rule with two intervals. Simpson's rule requires even number of intervals, but with two intervals (n=2), the formula is (h/3)[f(0) +4f(0.5)+f(1)] where h=(1-0)/2=0.5.

So h=0.5, f(0)=0.25, f(0.5)=0.5, f(1)=0.75.

So Simpson's rule gives (0.5/3)[0.25 +4*0.5 +0.75] = (0.5/3)[0.25 +2 +0.75] = (0.5/3)(3) =0.5. So Simpson's rule also gives 0.5. So that's consistent. Therefore, the exact answer is indeed 1/2. So the integral is 1/2. Therefore, the exact answer is 1/2, and the numerical approximation is 0.5. So the problem is solved.
</think>

{"answer": "\\frac{1}{2}", "numerical_answer": "0.5000000000"}