Let's compute the integral:
\[
I = \int_0^\infty \frac{\tanh(x)}{e^x}\,dx
\]

### Step 1: Express \(\tanh(x)\) in terms of exponentials

Recall:
\[
\tanh(x) = \frac{e^x - e^{-x}}{e^x + e^{-x}}
\]

So,
\[
\frac{\tanh(x)}{e^x} = \frac{e^x - e^{-x}}{e^x + e^{-x}}\cdot \frac{1}{e^x} = \frac{1 - e^{-2x}}{e^x + e^{-x}}
\]

But let's simplify more carefully:

\[
e^x + e^{-x} = e^x(1 + e^{-2x})
\]
So,
\[
\frac{\tanh(x)}{e^x} = \frac{e^x - e^{-x}}{e^x + e^{-x}} \cdot \frac{1}{e^x} = \frac{e^x - e^{-x}}{e^x(e^x + e^{-x})}
= \frac{1 - e^{-2x}}{e^x + e^{-x}}
\]
But it might be easier to rewrite as:

Because \(e^x + e^{-x} = 2\cosh(x)\),
\[
\frac{\tanh(x)}{e^x} = \frac{\sinh(x)}{\cosh(x)e^x}
\]
But \(\sinh(x) = \frac{e^x - e^{-x}}{2}\):
\[
\frac{\sinh(x)}{e^x} = \frac{e^x - e^{-x}}{2e^x} = \frac{1 - e^{-2x}}{2}
\]
So,
\[
\frac{\tanh(x)}{e^x} = \frac{\sinh(x)}{\cosh(x)e^x} = \frac{1}{2}\cdot\frac{1 - e^{-2x}}{\cosh(x)}
\]

But maybe let's use the series for \(\tanh(x)\):
\[
\tanh(x) = 2\sum_{n=1}^\infty \frac{(-1)^{n+1}}{2n-1}e^{-(2n-1)x}
\]
So,
\[
\frac{\tanh(x)}{e^x} = 2\sum_{n=1}^\infty \frac{(-1)^{n+1}}{2n-1}e^{-(2n-1)x} \cdot e^{-x}
= 2\sum_{n=1}^\infty \frac{(-1)^{n+1}}{2n-1}e^{-2nx}
\]

### Step 2: Integrate term by term

\[
I = \int_0^\infty \frac{\tanh(x)}{e^x} dx = 2\sum_{n=1}^\infty \frac{(-1)^{n+1}}{2n-1} \int_0^\infty e^{-2n x} dx
\]

**Integral:**
\[
\int_0^\infty e^{-2n x} dx = \left[ -\frac{1}{2n} e^{-2n x} \right]_0^\infty
= 0 + \frac{1}{2n} = \frac{1}{2n}
\]

So our sum becomes:
\[
I = 2\sum_{n=1}^\infty \frac{(-1)^{n+1}}{2n-1} \cdot \frac{1}{2n}
= \sum_{n=1}^\infty \frac{(-1)^{n+1}}{n(2n-1)}
\]

### Step 3: Further simplification and closed form

Let us expand:
\[
\frac{1}{n(2n-1)} 
= \frac{A}{n} + \frac{B}{2n-1}
\]
Solving,
\[
1 = A(2n-1) + B n \implies A(2n-1) + B n = 1
\]
Match coefficients:
- \(n\): \(2A + B = 0\)
- constant: \(-A = 1\)

Thus, \(A = -1\), then \(2(-1) + B = 0 \implies B = 2\)

So,
\[
\frac{1}{n(2n-1)} = -\frac{1}{n} + \frac{2}{2n-1}
\]

Therefore,
\[
I = \sum_{n=1}^\infty (-1)^{n+1} \left[ -\frac{1}{n} + \frac{2}{2n-1} \right ]
= -\sum_{n=1}^\infty \frac{(-1)^{n+1}}{n} + 2\sum_{n=1}^\infty \frac{(-1)^{n+1}}{2n-1}
\]

The first sum is the alternating harmonic series, and the second is the alternating odd harmonic series.

Recall:
- \(\sum_{n=1}^\infty \frac{(-1)^{n+1}}{n} = \ln 2\)
- \(\sum_{n=1}^\infty \frac{(-1)^{n+1}}{2n-1} = \frac{\pi}{4}\) (see e.g., Fourier series for arctan)

So,
\[
I = -\ln 2 + 2 \cdot \frac{\pi}{4}
= -\ln 2 + \frac{\pi}{2}
\]

### Step 4: Numerical evaluation
Let us compute:
\[
I = \frac{\pi}{2} - \ln 2
\]

- \(\pi \approx 3.1415926536\)
- \(\frac{\pi}{2} \approx 1.5707963268\)
- \(\ln 2 \approx 0.6931471806\)
Thus,
\[
I \approx 1.5707963268 - 0.6931471806 = 0.8776491462
\]

### Final JSON Output

```json
{"answer": "\\frac{\\pi}{2} - \\ln 2", "numerical_answer": "0.8776491462"}
```