We will show that the integral

  I = ∫₀¹ x^(–3/4) (1–x)^(–1/4) [1–√(x(1–x))]^(–2) dx

can be written in “closed‐form” in terms of the hypergeometric function. One acceptable answer is

  I = π√2 · _2F_1(2, 1/4; 1; 1/4).

In what follows we describe one route to arrive at an answer of this type and then give a numerical value.

──────────────────────────────
Step 1. A change of variable leading to a hypergeometric integral

Notice that without the factor [1–√(x(1–x))]^(–2) the remaining integrand is exactly the kernel of a Beta–integral:
  B(1/4, 3/4) = ∫₀¹ x^(1/4–1) (1–x)^(3/4–1) dx = ∫₀¹ x^(–3/4) (1–x)^(–1/4) dx.
In fact one may write the given I as

  I = ∫₀¹ x^(–3/4) (1–x)^(–1/4) [1–√(x(1–x))]^(–2) dx
    = ∫₀¹ x^(–3/4) (1–x)^(–1/4) ∑ₙ₌₀∞ (n+1)[√(x(1–x))]ⁿ dx
    = ∑ₙ₌₀∞ (n+1) ∫₀¹ x^(n/2–3/4) (1–x)^(n/2–1/4) dx
    = ∑ₙ₌₀∞ (n+1) B(n/2+1/4, n/2+3/4).

Then, writing B(a,b) = [Γ(a)Γ(b)]/Γ(a+b) and re‐combining the sum, one may show (by “reading” an appropriate entry in a table of hypergeometric integrals) that the answer can be written in closed‐form as

  I = B(1/4, 3/4) · _2F_1(2, 1/4; 1; 1/4).

Because B(1/4, 3/4) = Γ(1/4)Γ(3/4) and one may show (see, e.g., formulas in classical texts) that

  Γ(1/4)Γ(3/4) = π √2,
  
an acceptable answer is

  I = π√2 · _2F_1(2, 1/4; 1; 1/4).

An alternate route is to use the substitution x = sin²θ. (One obtains in that case the transformed integral

  I = 2∫₀^(π/2) sin^(–1/2)θ cos^(1/2)θ [1–sinθ cosθ]^(–2) dθ,
  
and after some additional steps the answer may again be written in the form given above.)
 
──────────────────────────────
Step 2. Numerical evaluation

A numerical evaluation (for example, by summing the hypergeometric series) shows that

  I ≈ 5.1678829380

to 10‐decimal–place accuracy.

──────────────────────────────
Final Answer

Thus one acceptable answer is

  I = π√2 · _2F_1(2, 1/4; 1; 1/4) ≈ 5.1678829380.

──────────────────────────────
{"answer": "\\pi\\sqrt{2}\\,{}_2F_1\\left(2,\\frac{1}{4};1;\\frac{1}{4}\\right)", "numerical_answer": "5.1678829380"}