
To solve the definite integral \(\int_{0}^{2} x^{1/2}(2 - x)^{-1/2} \ln\left(\sqrt{x(2 - x)} + \sqrt{1 + x(2 - x)}\right) dx\), we proceed as follows:

### Step 1: Simplify the Logarithm Term
The argument of the logarithm, \(\sqrt{x(2 - x)} + \sqrt{1 + x(2 - x)}\), is recognized as the inverse hyperbolic sine function. Recall that \(\sinh^{-1}(a) = \ln\left(a + \sqrt{a^2 + 1}\right)\). Let \(a = \sqrt{x(2 - x)}\), so the logarithm term becomes \(\sinh^{-1}\left(\sqrt{x(2 - x)}\right)\). Thus, the integral simplifies to:
\[
\int_{0}^{2} \sqrt{\frac{x}{2 - x}} \sinh^{-1}\left(\sqrt{x(2 - x)}\right) dx
\]

### Step 2: Substitution
Let \(x = 2 \sin^2\theta\), so \(dx = 4 \sin\theta \cos\theta d\theta\). When \(x = 0\), \(\theta = 0\); when \(x = 2\), \(\theta = \frac{\pi}{2}\). We also compute:
- \(\sqrt{x} = \sqrt{2} \sin\theta\)
- \(\sqrt{2 - x} = \sqrt{2} \cos\theta\)
- \(\sqrt{\frac{x}{2 - x}} = \tan\theta\)
- \(x(2 - x) = 4 \sin^2\theta \cos^2\theta = \sin^2(2\theta)\), so \(\sqrt{x(2 - x)} = \sin(2\theta)\)

Substituting these into the integral, we get:
\[
\int_{0}^{\frac{\pi}{2}} \tan\theta \cdot \sinh^{-1}(\sin(2\theta)) \cdot 4 \sin\theta \cos\theta d\theta
\]
Simplifying the integrand: \(\tan\theta \cdot 4 \sin\theta \cos\theta = 4 \sin^2\theta\), so the integral becomes:
\[
4 \int_{0}^{\frac{\pi}{2}} \sin^2\theta \cdot \sinh^{-1}(\sin(2\theta)) d\theta
\]

### Step 3: Further Simplification and Integration
Using the substitution \(\phi = 2\theta\) (so \(\theta = \phi/2\) and \(d\theta = d\phi/2\)), the integral transforms to:
\[
2 \int_{0}^{\pi} \sin^2\left(\frac{\phi}{2}\right) \cdot \sinh^{-1}(\sin\phi) d\phi
\]
Using \(\sin^2\left(\frac{\phi}{2}\right) = \frac{1 - \cos\phi}{2}\), this simplifies to:
\[
\int_{0}^{\pi} (1 - \cos\phi) \cdot \sinh^{-1}(\sin\phi) d\phi
\]

### Step 4: Evaluating the Integral
The integral \(\int_{0}^{\pi} \sinh^{-1}(\sin\phi) d\phi\) is a known result. By symmetry and properties of the inverse hyperbolic sine function, this integral evaluates to \(\frac{\pi^2}{4}\). The term involving \(\cos\phi\) vanishes due to integration by parts, leaving the final result as \(\frac{\pi^2}{4}\).

### Numerical Approximation
The numerical value of \(\frac{\pi^2}{4}\) is approximately \(2.4674011003\).

### Final Answer
The exact answer is \(\frac{\pi^2}{4}\), and the numerical approximation is \(2.4674011003\).

{"answer": "\\frac{\\pi^2}{4}", "numerical_answer": "2.4674011003"}