To solve the definite integral 

\[
\int_{0}^{1} x^{-1/2} \left[1 - \sqrt{x(1 - x)}\right]^{-2} \, dx,
\]

we will follow these steps:

### Step 1: Simplify the Integrand
First, let's rewrite the integrand for clarity:

\[
x^{-1/2} \left[1 - \sqrt{x(1 - x)}\right]^{-2} = \frac{1}{\sqrt{x} \left(1 - \sqrt{x(1 - x)}\right)^2}.
\]

### Step 2: Substitution
Let’s make the substitution \( x = \sin^2 \theta \). Then:

\[
dx = 2 \sin \theta \cos \theta \, d\theta,
\]

and the limits change as follows:
- When \( x = 0 \), \( \theta = 0 \).
- When \( x = 1 \), \( \theta = \frac{\pi}{2} \).

The integrand becomes:

\[
\frac{1}{\sin \theta \left(1 - \sqrt{\sin^2 \theta (1 - \sin^2 \theta)}\right)^2} \cdot 2 \sin \theta \cos \theta \, d\theta.
\]

Simplify the expression under the square root:

\[
\sqrt{\sin^2 \theta \cos^2 \theta} = \sin \theta \cos \theta.
\]

So the integrand simplifies to:

\[
\frac{2 \cos \theta}{\left(1 - \sin \theta \cos \theta\right)^2} \, d\theta.
\]

### Step 3: Further Simplification
Now, the integral becomes:

\[
2 \int_{0}^{\pi/2} \frac{\cos \theta}{\left(1 - \sin \theta \cos \theta\right)^2} \, d\theta.
\]

Let’s use the identity \( \sin \theta \cos \theta = \frac{1}{2} \sin 2\theta \):

\[
2 \int_{0}^{\pi/2} \frac{\cos \theta}{\left(1 - \frac{1}{2} \sin 2\theta\right)^2} \, d\theta = 8 \int_{0}^{\pi/2} \frac{\cos \theta}{\left(2 - \sin 2\theta\right)^2} \, d\theta.
\]

### Step 4: Another Substitution
Let \( u = \theta \), then \( du = d\theta \). However, this doesn't simplify the integral directly. Instead, let’s consider the substitution \( t = \tan \theta \). Then:

\[
\sin \theta = \frac{t}{\sqrt{1 + t^2}}, \quad \cos \theta = \frac{1}{\sqrt{1 + t^2}}, \quad d\theta = \frac{dt}{1 + t^2}.
\]

The integral becomes:

\[
8 \int_{0}^{\infty} \frac{\frac{1}{\sqrt{1 + t^2}}}{\left(2 - \frac{2t}{1 + t^2}\right)^2} \cdot \frac{dt}{1 + t^2} = 8 \int_{0}^{\infty} \frac{1}{\left(2(1 + t^2) - 2t\right)^2} \, dt.
\]

Simplify the denominator:

\[
2(1 + t^2) - 2t = 2t^2 - 2t + 2 = 2(t^2 - t + 1).
\]

So the integral becomes:

\[
8 \int_{0}^{\infty} \frac{1}{4(t^2 - t + 1)^2} \, dt = 2 \int_{0}^{\infty} \frac{1}{(t^2 - t + 1)^2} \, dt.
\]

### Step 5: Partial Fractions and Residues
The integral \( \int \frac{1}{(t^2 - t + 1)^2} \, dt \) can be evaluated using complex analysis or by completing the square and using standard techniques. Here, we’ll use the result from standard tables or symbolic computation:

\[
\int \frac{1}{(t^2 - t + 1)^2} \, dt = \frac{2t - 1}{3(t^2 - t + 1)} + \frac{2\sqrt{3}}{9} \arctan\left(\frac{2t - 1}{\sqrt{3}}\right) + C.
\]

Evaluating from \( 0 \) to \( \infty \):

\[
\left. \frac{2t - 1}{3(t^2 - t + 1)} \right|_{0}^{\infty} = 0 - \left(-\frac{1}{3}\right) = \frac{1}{3},
\]

and

\[
\left. \frac{2\sqrt{3}}{9} \arctan\left(\frac{2t - 1}{\sqrt{3}}\right) \right|_{0}^{\infty} = \frac{2\sqrt{3}}{9} \left(\frac{\pi}{2} - \left(-\frac{\pi}{6}\right)\right) = \frac{2\sqrt{3}}{9} \cdot \frac{2\pi}{3} = \frac{4\sqrt{3}\pi}{27}.
\]

Thus,

\[
\int_{0}^{\infty} \frac{1}{(t^2 - t + 1)^2} \, dt = \frac{1}{3} + \frac{4\sqrt{3}\pi}{27}.
\]

Multiplying by 2:

\[
2 \left(\frac{1}{3} + \frac{4\sqrt{3}\pi}{27}\right) = \frac{2}{3} + \frac{8\sqrt{3}\pi}{27}.
\]

### Step 6: Final Answer
The exact value of the integral is:

\[
\frac{2}{3} + \frac{8\sqrt{3}\pi}{27}.
\]

### Numerical Approximation
Calculating the numerical value:

\[
\frac{2}{3} + \frac{8\sqrt{3}\pi}{27} \approx 0.6666666667 + 1.612103638 \approx 2.278770305.
\]

Rounding to 10 decimal places:

\[
2.2787703046.
\]

### JSON Output
```json
{"answer": "\\frac{2}{3} + \\frac{8\\sqrt{3}\\pi}{27}", "numerical_answer": "2.2787703046"}
```