<think>
Okay, so I need to compute the definite integral of cos(x) divided by (1 + e^(-1/x)) from -1 to 1. Hmm, let me start by understanding the integrand. The function is cos(x)/(1 + e^(-1/x)). First, I should check if there are any symmetries or substitutions that can simplify the integral.

Wait, the limits are from -1 to 1. Maybe there's a substitution that can exploit the interval's symmetry. Let me consider substituting x with -t. Let’s let t = -x. Then when x = -1, t = 1, and when x = 1, t = -1. The differential dx becomes -dt. So the integral becomes the integral from t=1 to t=-1 of cos(-t)/(1 + e^(-1/(-t))) * (-dt). Flipping the limits back to 1 to -1 would remove the negative sign. So, integral from -1 to 1 becomes integral from 1 to -1 with substitution, but I need to reverse the limits again. Let me write it properly.

Original integral: I = ∫_{-1}^1 [cos x / (1 + e^(-1/x))] dx

Substitute x = -t, dx = -dt. Then:

I = ∫_{t=1}^{t=-1} [cos(-t) / (1 + e^(-1/(-t)))] (-dt) = ∫_{-1}^1 [cos(t) / (1 + e^(1/t))] dt

Because cos(-t) = cos(t), and -1/(-t) is 1/t. So the integral becomes ∫_{-1}^1 [cos(t)/(1 + e^(1/t))] dt. Let me rename t back to x for clarity:

I = ∫_{-1}^1 [cos(x)/(1 + e^(1/x))] dx

Now, if I add the original integral I and this transformed integral, maybe something cancels. Let's denote the original as I and the transformed as I'. Wait, but actually, they are the same integral but written differently. Wait, no. Wait, the original integrand is cos(x)/(1 + e^(-1/x)), and after substitution, it's cos(x)/(1 + e^(1/x)). So if I add them:

I + I' = ∫_{-1}^1 [cos(x)/(1 + e^(-1/x)) + cos(x)/(1 + e^(1/x))] dx

Let me compute the sum of the two fractions. Let’s compute 1/(1 + e^(-1/x)) + 1/(1 + e^(1/x)).

Let’s common denominator. The denominators are (1 + e^(-1/x)) and (1 + e^(1/x)). Multiply numerator and denominator appropriately:

[ (1 + e^(1/x)) + (1 + e^(-1/x)) ] / [ (1 + e^(-1/x))(1 + e^(1/x)) ]

Simplify numerator: 1 + e^(1/x) + 1 + e^(-1/x) = 2 + e^(1/x) + e^(-1/x)

Denominator: (1 + e^(-1/x))(1 + e^(1/x)) = 1 + e^(1/x) + e^(-1/x) + e^(0) = 1 + e^(1/x) + e^(-1/x) + 1 = 2 + e^(1/x) + e^(-1/x)

So numerator and denominator are the same. Therefore, the sum is 1. So I + I' = ∫_{-1}^1 cos(x) * 1 dx = ∫_{-1}^1 cos(x) dx

But wait, the sum of the two integrals I and I' is equal to the integral of cos(x) from -1 to 1. But since I and I' are the same integral? Wait, no. Wait, I is the original integral, and I' is the integral after substitution. But actually, when we did the substitution, we found that I = ∫_{-1}^1 [cos(x)/(1 + e^(1/x))] dx. So the original I is ∫_{-1}^1 [cos(x)/(1 + e^(-1/x))] dx, and the transformed I' is ∫_{-1}^1 [cos(x)/(1 + e^(1/x))] dx. So adding them gives:

I + I' = ∫_{-1}^1 cos(x) [1/(1 + e^(-1/x)) + 1/(1 + e^(1/x))] dx = ∫_{-1}^1 cos(x) dx

But we just saw that the term in the brackets simplifies to 1, so I + I' = ∫_{-1}^1 cos(x) dx. But the integral of cos(x) is sin(x), so evaluated from -1 to 1, that's sin(1) - sin(-1) = 2 sin(1). Therefore, I + I' = 2 sin(1). But here's the thing: I' is actually equal to the original integral I? Wait, no. Wait, I' is the integral of cos(x)/(1 + e^(1/x)) dx from -1 to 1, which is different from I. So I and I' are two different integrals. But if we can relate them, maybe we can find that I = I', but that's not obvious. Wait, but let's check if the integrand of I' can be related to the original integrand.

Wait, in the original integral, the denominator is 1 + e^(-1/x). In I', it's 1 + e^(1/x). Let me see if there's a relationship between them. Let's note that 1/(1 + e^(-1/x)) = e^(1/x)/(1 + e^(1/x)). Because:

1/(1 + e^(-1/x)) = e^(1/x)/(e^(1/x) + 1) = e^(1/x)/(1 + e^(1/x))

So, the original integrand is cos(x) * e^(1/x)/(1 + e^(1/x)). Therefore, I = ∫_{-1}^1 [cos(x) e^(1/x) / (1 + e^(1/x))] dx. Then, if we add I and I', which is ∫ [cos(x)/(1 + e^(1/x))] dx, we get:

I + I' = ∫_{-1}^1 cos(x) [e^(1/x)/(1 + e^(1/x)) + 1/(1 + e^(1/x))] dx = ∫_{-1}^1 cos(x) [ (e^(1/x) + 1)/(1 + e^(1/x)) ] dx = ∫_{-1}^1 cos(x) dx = 2 sin(1)

Therefore, I + I' = 2 sin(1). But if we can find a relationship between I and I', maybe they are equal? Let's check if I = I'. Let's see:

Original I: ∫_{-1}^1 [cos(x)/(1 + e^(-1/x))] dx

I': ∫_{-1}^1 [cos(x)/(1 + e^(1/x))] dx

But if we make a substitution in I: let t = -x, as before. Then, in the original integral, substituting x = -t, we get:

I = ∫_{1}^{-1} [cos(-t)/(1 + e^(-1/(-t)))] (-dt) = ∫_{-1}^1 [cos(t)/(1 + e^(1/t))] dt = I'

Therefore, I = I'. Therefore, since I = I', then 2I = 2 sin(1), so I = sin(1). Therefore, the integral is equal to sin(1). That's the analytical result.

Wait, that seems too straightforward. Let me verify this again. So, by substituting x = -t in the original integral, we found that I = I', which is the integral of cos(x)/(1 + e^(1/x)) dx from -1 to 1. Then, when we add I and I', we get 2 sin(1). But since I = I', then 2I = 2 sin(1), so I = sin(1). Therefore, the exact answer is sin(1). Let me check this with a numerical approximation.

But let's also check if there are any issues with the integrand. The function 1/(1 + e^(-1/x)) has a potential problem at x = 0. Because as x approaches 0 from the positive side, 1/x approaches +infty, so e^(-1/x) approaches 0, so the denominator approaches 1. As x approaches 0 from the negative side, 1/x approaches -infty, so e^(-1/x) approaches e^{infty} which is infinity, so the denominator approaches infinity, so the integrand approaches 0. However, at x=0, the function is undefined. But the original integral is from -1 to 1, so we need to check if the integral is improper at x=0. However, the integrand near x=0 from the left (negative x) approaches 0, and from the right (positive x) approaches cos(0)/1 = 1. So the integrand is continuous except at x=0. But since the integral is from -1 to 1, and the integrand has a discontinuity at 0, we need to consider the integral as an improper integral, splitting it into two parts: from -1 to 0 and from 0 to 1. However, since the integrand approaches 0 from the left and 1 from the right, the integral over an interval including 0 would still converge. Let me check the behavior near x=0.

For x approaching 0 from the positive side (x → 0+), 1/x → +infty, so e^(-1/x) → 0, so the integrand becomes cos(x)/1 ≈ cos(0) = 1. So near 0+, the integrand is approximately 1, which is integrable. For x approaching 0 from the negative side (x → 0-), 1/x → -infty, so e^(-1/x) = e^{positive large} → +infty, so the integrand becomes cos(x)/(1 + something very big) ≈ 0. So the integrand is continuous from the left and right, but at x=0, it's undefined. However, the integral from -1 to 1 is the sum of the integral from -1 to 0 and from 0 to 1. Both integrals are proper except at x=0. So we can write the integral as the limit a→0- ∫_{-1}^a [cos(x)/(1 + e^(-1/x))] dx + limit b→0+ ∫_{b}^1 [cos(x)/(1 + e^(-1/x))] dx. But since near 0 from the left, the integrand approaches 0, and from the right approaches 1, the integral over [0,1] would have a finite value. But according to our previous analysis, the integral is sin(1). Let's compute the numerical value of sin(1) to check.

Sin(1) in radians is approximately 0.8414709848. Let me compute the integral numerically to verify. If I compute ∫_{-1}^1 cos(x)/(1 + e^(-1/x)) dx numerically, it should be approximately 0.8414709848. Let me check with a calculator or approximate.

Alternatively, since the integrand is symmetric in a way that allows the integral to be simplified to sin(1), the analytical result is sin(1). Therefore, the exact answer is sin(1), and the numerical approximation is approximately 0.8414709848.

But wait, let me confirm this with a substitution. Let's split the integral into two parts: from -1 to 0 and from 0 to 1.

Let’s consider I = ∫_{-1}^1 [cos(x)/(1 + e^(-1/x})] dx = ∫_{-1}^0 [cos(x)/(1 + e^(-1/x})] dx + ∫_{0}^1 [cos(x)/(1 + e^(-1/x})] dx

For the integral from -1 to 0, let’s substitute x = -t, so t ranges from 1 to 0. Then dx = -dt, and the integral becomes ∫_{1}^{0} [cos(-t)/(1 + e^(-1/(-t)))] (-dt) = ∫_{0}^{1} [cos(t)/(1 + e^{1/t})] dt

So the integral from -1 to 0 is equal to ∫_{0}^{1} [cos(t)/(1 + e^{1/t})] dt. Therefore, the original integral I is equal to ∫_{0}^{1} [cos(t)/(1 + e^{1/t})] dt + ∫_{0}^1 [cos(x)/(1 + e^{-1/x})] dx. Let’s rename variables in the first integral to x:

I = ∫_{0}^1 [cos(x)/(1 + e^{1/x}) + cos(x)/(1 + e^{-1/x})] dx

But as before, the sum inside the integral is cos(x) [1/(1 + e^{1/x}) + 1/(1 + e^{-1/x})] = cos(x) [1/(1 + e^{1/x}) + e^{1/x}/(1 + e^{1/x})] = cos(x) [ (1 + e^{1/x}) / (1 + e^{1/x}) ] = cos(x). Therefore, I = ∫_{0}^1 cos(x) dx = sin(1) - sin(0) = sin(1). So this confirms the analytical result. Therefore, the integral is indeed sin(1).

So the exact answer is sin(1), and the numerical approximation is approximately 0.8414709848, which to 10 decimal places is 0.8414709848. Let me check with a calculator: sin(1 radian) is approximately 0.8414709848078965, so rounding to 10 decimal places would be 0.8414709848.

Therefore, the final answer is {"answer": "\\sin(1)", "numerical_answer": 0.8414709848}
</think>

{"answer": "\\sin(1)", "numerical_answer": 0.8414709848}