Let's consider the integral:
\[
I = \int_0^{2\pi} |1 + 2 \sin x| \, dx
\]

**Step 1: Find the points where \(1 + 2 \sin x = 0\) in \([0, 2\pi]\)**

Set \(1 + 2\sin x = 0\):

\[
2 \sin x = -1 \implies \sin x = -\frac{1}{2}
\]
In \([0, 2\pi]\), this has two solutions:
\[
x_1 = \arcsin\left(-\frac{1}{2}\right) = \frac{7\pi}{6}
\]
and
\[
x_2 = 2\pi - \arcsin\left(\frac{1}{2}\right) = \frac{11\pi}{6}
\]

**Step 2: Break the integral into intervals where the sign of \(1 + 2\sin x\) doesn't change**

The sign changes at \(x_1 = \frac{7\pi}{6}\) and \(x_2 = \frac{11\pi}{6}\).

Test values:
- For \(x \in [0, \frac{7\pi}{6})\): Use \(x=0\), \(1 + 2\sin 0 = 1 > 0\)
- For \(x \in (\frac{7\pi}{6}, \frac{11\pi}{6})\): Use \(x= \frac{3\pi}{2}\), \(1 + 2\sin \frac{3\pi}{2} = 1 + 2(-1) = -1 < 0\)
- For \(x \in (\frac{11\pi}{6}, 2\pi]\): Use \(x=2\pi\), \(1 + 2 \sin 2\pi = 1 > 0\)

So,
\[
I = \int_0^{\frac{7\pi}{6}} (1 + 2\sin x)\, dx + \int_{\frac{7\pi}{6}}^{\frac{11\pi}{6}} -(1 + 2\sin x)\, dx + \int_{\frac{11\pi}{6}}^{2\pi} (1 + 2\sin x)\, dx
\]

\[
= \int_0^{\frac{7\pi}{6}} (1 + 2\sin x)\, dx - \int_{\frac{7\pi}{6}}^{\frac{11\pi}{6}} (1 + 2\sin x)\, dx + \int_{\frac{11\pi}{6}}^{2\pi} (1 + 2\sin x)\, dx
\]

**Step 3: Compute the antiderivative of \(1 + 2\sin x\)**

\[
\int (1 + 2\sin x) dx = x - 2\cos x + C
\]

**Step 4: Compute each part**

- First part: \(A = \int_0^{\frac{7\pi}{6}} (1 + 2\sin x) dx\)
- Second part: \(B = \int_{\frac{7\pi}{6}}^{\frac{11\pi}{6}} (1 + 2\sin x) dx\)
- Third part: \(C = \int_{\frac{11\pi}{6}}^{2\pi} (1 + 2\sin x) dx\)

Compute:

\[
A = \left[x - 2\cos x \right]_0^{\frac{7\pi}{6}} = \left(\frac{7\pi}{6} - 2\cos\frac{7\pi}{6}\right) - (0 - 2\cos 0)
\]
\[
= \frac{7\pi}{6} - 2\cos\frac{7\pi}{6} + 2
\]

Similarly,
\[
B = \left[x - 2\cos x \right]_{\frac{7\pi}{6}}^{\frac{11\pi}{6}} = \left(\frac{11\pi}{6} - 2\cos\frac{11\pi}{6}\right) - \left(\frac{7\pi}{6} - 2\cos\frac{7\pi}{6}\right)
\]
\[
= \frac{4\pi}{6} - 2\left(\cos\frac{11\pi}{6} - \cos\frac{7\pi}{6}\right) = \frac{2\pi}{3} - 2\left(\cos\frac{11\pi}{6} - \cos\frac{7\pi}{6}\right)
\]

And,
\[
C = \left[x - 2\cos x \right]_{\frac{11\pi}{6}}^{2\pi} = \left(2\pi - 2\cos 2\pi\right) - \left(\frac{11\pi}{6} - 2\cos\frac{11\pi}{6}\right)
\]
\[
= 2\pi - 2\cos 2\pi - \frac{11\pi}{6} + 2\cos\frac{11\pi}{6}
\]

Now, the value of the definite integral is:
\[
I = A - B + C
\]

**Step 5: Compute the cosines**

Recall:
\[
\cos\left(\frac{7\pi}{6}\right) = -\cos\left(\frac{\pi}{6}\right) = -\frac{\sqrt{3}}{2}
\]
\[
\cos\left(\frac{11\pi}{6}\right) = \cos\left(2\pi - \frac{\pi}{6}\right) = \cos\left(\frac{\pi}{6}\right) = \frac{\sqrt{3}}{2}
\]

\[
\cos(0) = 1,\quad \cos(2\pi) = 1
\]

So, substitute these in:

First,
\[
A = \frac{7\pi}{6} - 2\left(-\frac{\sqrt{3}}{2}\right) + 2 = \frac{7\pi}{6} + \sqrt{3} + 2
\]

Second,
\[
B = \frac{2\pi}{3} - 2 \left(\frac{\sqrt{3}}{2} - \left(-\frac{\sqrt{3}}{2}\right) \right) = \frac{2\pi}{3} - 2 (\sqrt{3})
\]

Third,
\[
C = 2\pi - 2(1) - \frac{11\pi}{6} + 2\left(\frac{\sqrt{3}}{2}\right) = (2\pi - \frac{11\pi}{6}) - 2 + \sqrt{3}
\]
\[
2\pi - \frac{11\pi}{6} = \frac{12\pi}{6} - \frac{11\pi}{6} = \frac{\pi}{6}
\]
So,
\[
C = \frac{\pi}{6} - 2 + \sqrt{3}
\]

Now, plug these into the expression for \(I\):

\[
I = A - B + C = \left(\frac{7\pi}{6} + \sqrt{3} + 2\right) - \left(\frac{2\pi}{3} - 2\sqrt{3}\right) + \left(\frac{\pi}{6} - 2 + \sqrt{3}\right)
\]

Expand:

\[
= \frac{7\pi}{6} + \sqrt{3} + 2 - \frac{2\pi}{3} + 2\sqrt{3} + \frac{\pi}{6} - 2 + \sqrt{3}
\]

Group like terms:

- \(\pi\) terms: \(\frac{7\pi}{6} - \frac{2\pi}{3} + \frac{\pi}{6}\)
- \(\sqrt{3}\) terms: \(\sqrt{3} + 2\sqrt{3} + \sqrt{3}\)
- Constants: \(2 - 2 = 0\)

Let's combine:

1. \(\frac{7\pi}{6} - \frac{2\pi}{3} + \frac{\pi}{6}\)

Note: \(\frac{2\pi}{3} = \frac{4\pi}{6}\)
So:

\[
\frac{7\pi}{6} - \frac{4\pi}{6} + \frac{\pi}{6} = \frac{(7-4+1)\pi}{6} = \frac{4\pi}{6} = \frac{2\pi}{3}
\]

2. \(\sqrt{3} + 2\sqrt{3} + \sqrt{3} = 4\sqrt{3}\)

So the sum is:

\[
I = \frac{2\pi}{3} + 4\sqrt{3}
\]

**Step 6: Numerical approximation (10 decimal places)**

- Use \(\pi \approx 3.1415926536\)
- \(\sqrt{3} \approx 1.7320508076\)
- Compute \(\frac{2\pi}{3} \approx \frac{2 \times 3.1415926536}{3} = 2.0943951024\)
- Compute \(4\sqrt{3} = 4 \times 1.7320508076 = 6.9282032304\)

Sum:

\[
I \approx 2.0943951024 + 6.9282032304 = 9.0225983328
\]

**Final JSON answer:**
```json
{"answer": "\\frac{2\\pi}{3} + 4\\sqrt{3}", "numerical_answer": "9.0225983328"}
```