To solve the definite integral \(\int_1^e x (\log x)^2 \, dx\), we will use integration by parts. Let's denote \(u = (\log x)^2\) and \(dv = x \, dx\).

### Step 1: Integration by Parts
Recall the formula for integration by parts:
\[
\int u \, dv = uv - \int v \, du
\]

First, we need to find \(du\) and \(v\):
\[
u = (\log x)^2 \implies du = 2 \log x \cdot \frac{1}{x} \, dx = \frac{2 \log x}{x} \, dx
\]
\[
dv = x \, dx \implies v = \frac{x^2}{2}
\]

Now, apply the integration by parts formula:
\[
\int_1^e x (\log x)^2 \, dx = \left[ \frac{x^2}{2} (\log x)^2 \right]_1^e - \int_1^e \frac{x^2}{2} \cdot \frac{2 \log x}{x} \, dx
\]

Simplify the integral:
\[
= \left[ \frac{x^2}{2} (\log x)^2 \right]_1^e - \int_1^e x \log x \, dx
\]

### Step 2: Evaluate the Boundary Term
Evaluate the boundary term:
\[
\left[ \frac{x^2}{2} (\log x)^2 \right]_1^e = \frac{e^2}{2} (\log e)^2 - \frac{1^2}{2} (\log 1)^2 = \frac{e^2}{2} \cdot 1^2 - \frac{1}{2} \cdot 0 = \frac{e^2}{2}
\]

### Step 3: Solve the Remaining Integral
Now, we need to solve \(\int_1^e x \log x \, dx\). Again, use integration by parts with \(u = \log x\) and \(dv = x \, dx\):
\[
u = \log x \implies du = \frac{1}{x} \, dx
\]
\[
dv = x \, dx \implies v = \frac{x^2}{2}
\]

Apply the integration by parts formula:
\[
\int_1^e x \log x \, dx = \left[ \frac{x^2}{2} \log x \right]_1^e - \int_1^e \frac{x^2}{2} \cdot \frac{1}{x} \, dx
\]
\[
= \left[ \frac{x^2}{2} \log x \right]_1^e - \int_1^e \frac{x}{2} \, dx
\]

Evaluate the boundary term:
\[
\left[ \frac{x^2}{2} \log x \right]_1^e = \frac{e^2}{2} \log e - \frac{1^2}{2} \log 1 = \frac{e^2}{2} \cdot 1 - \frac{1}{2} \cdot 0 = \frac{e^2}{2}
\]

Evaluate the remaining integral:
\[
\int_1^e \frac{x}{2} \, dx = \frac{1}{2} \int_1^e x \, dx = \frac{1}{2} \left[ \frac{x^2}{2} \right]_1^e = \frac{1}{2} \left( \frac{e^2}{2} - \frac{1}{2} \right) = \frac{e^2}{4} - \frac{1}{4}
\]

Combine the results:
\[
\int_1^e x \log x \, dx = \frac{e^2}{2} - \left( \frac{e^2}{4} - \frac{1}{4} \right) = \frac{e^2}{2} - \frac{e^2}{4} + \frac{1}{4} = \frac{e^2}{4} + \frac{1}{4}
\]

### Step 4: Combine All Parts
Now, combine all parts to get the final result:
\[
\int_1^e x (\log x)^2 \, dx = \frac{e^2}{2} - \left( \frac{e^2}{4} + \frac{1}{4} \right) = \frac{e^2}{2} - \frac{e^2}{4} - \frac{1}{4} = \frac{e^2}{4} - \frac{1}{4}
\]

### Step 5: Numerical Approximation
Evaluate the numerical approximation:
\[
\frac{e^2}{4} - \frac{1}{4} \approx \frac{7.38905609893065}{4} - \frac{1}{4} \approx 1.84726402473266 - 0.25 = 1.59726402473266
\]

### Final Answer
\[
\boxed{
\begin{aligned}
\text{"answer": "}\frac{e^2 - 1}{4}\text{"}, \\
\text{"numerical_answer": "1.5972640247"}
\end{aligned}
}
\]