To solve the definite integral \(\int_{-4}^4 |x^3 - x| \, dx\), we need to consider the behavior of the integrand \(|x^3 - x|\) over the interval \([-4, 4]\).

### Step 1: Analyze the integrand

The expression inside the absolute value is \(x^3 - x\). We need to determine where this expression changes sign within the interval \([-4, 4]\).

\[ x^3 - x = x(x^2 - 1) = x(x - 1)(x + 1) \]

The roots of \(x^3 - x\) are \(x = 0\), \(x = 1\), and \(x = -1\). These points divide the interval \([-4, 4]\) into four subintervals:
1. \([-4, -1]\)
2. \([-1, 0]\)
3. \([0, 1]\)
4. \([1, 4]\)

### Step 2: Determine the sign of \(x^3 - x\) in each subinterval

- For \(x \in [-4, -1]\), \(x^3 - x\) is positive.
- For \(x \in [-1, 0]\), \(x^3 - x\) is negative.
- For \(x \in [0, 1]\), \(x^3 - x\) is negative.
- For \(x \in [1, 4]\), \(x^3 - x\) is positive.

### Step 3: Split the integral

We split the integral into four parts based on the sign of \(x^3 - x\):

\[ \int_{-4}^4 |x^3 - x| \, dx = \int_{-4}^{-1} (x^3 - x) \, dx + \int_{-1}^{0} -(x^3 - x) \, dx + \int_{0}^{1} -(x^3 - x) \, dx + \int_{1}^{4} (x^3 - x) \, dx \]

### Step 4: Compute each integral

1. \(\int_{-4}^{-1} (x^3 - x) \, dx\):

\[ \int_{-4}^{-1} (x^3 - x) \, dx = \left[ \frac{x^4}{4} - \frac{x^2}{2} \right]_{-4}^{-1} \]

Evaluating at the bounds:

\[ \left( \frac{(-1)^4}{4} - \frac{(-1)^2}{2} \right) - \left( \frac{(-4)^4}{4} - \frac{(-4)^2}{2} \right) = \left( \frac{1}{4} - \frac{1}{2} \right) - \left( \frac{256}{4} - \frac{16}{2} \right) = \left( -\frac{1}{4} \right) - \left( 64 - 8 \right) = -\frac{1}{4} - 56 = -56.25 \]

2. \(\int_{-1}^{0} -(x^3 - x) \, dx\):

\[ \int_{-1}^{0} -(x^3 - x) \, dx = -\int_{-1}^{0} (x^3 - x) \, dx = -\left[ \frac{x^4}{4} - \frac{x^2}{2} \right]_{-1}^{0} \]

Evaluating at the bounds:

\[ -\left( \left( \frac{0^4}{4} - \frac{0^2}{2} \right) - \left( \frac{(-1)^4}{4} - \frac{(-1)^2}{2} \right) \right) = -\left( 0 - \left( \frac{1}{4} - \frac{1}{2} \right) \right) = -\left( -\frac{1}{4} \right) = \frac{1}{4} \]

3. \(\int_{0}^{1} -(x^3 - x) \, dx\):

\[ \int_{0}^{1} -(x^3 - x) \, dx = -\int_{0}^{1} (x^3 - x) \, dx = -\left[ \frac{x^4}{4} - \frac{x^2}{2} \right]_{0}^{1} \]

Evaluating at the bounds:

\[ -\left( \left( \frac{1^4}{4} - \frac{1^2}{2} \right) - \left( \frac{0^4}{4} - \frac{0^2}{2} \right) \right) = -\left( \left( \frac{1}{4} - \frac{1}{2} \right) - 0 \right) = -\left( -\frac{1}{4} \right) = \frac{1}{4} \]

4. \(\int_{1}^{4} (x^3 - x) \, dx\):

\[ \int_{1}^{4} (x^3 - x) \, dx = \left[ \frac{x^4}{4} - \frac{x^2}{2} \right]_{1}^{4} \]

Evaluating at the bounds:

\[ \left( \frac{4^4}{4} - \frac{4^2}{2} \right) - \left( \frac{1^4}{4} - \frac{1^2}{2} \right) = \left( \frac{256}{4} - \frac{16}{2} \right) - \left( \frac{1}{4} - \frac{1}{2} \right) = \left( 64 - 8 \right) - \left( -\frac{1}{4} \right) = 56 + \frac{1}{4} = 56.25 \]

### Step 5: Sum the integrals

\[ \int_{-4}^4 |x^3 - x| \, dx = -56.25 + \frac{1}{4} + \frac{1}{4} + 56.25 = 0.5 \]

### Step 6: Numerical approximation

The numerical approximation of \(0.5\) rounded to 10 decimal places is \(0.5000000000\).

### Final Answer

```json
{"answer": "\\frac{1}{2}", "numerical_answer": "0.5000000000"}
```