<think>
Okay, so I need to compute the definite integral from 0 to 1 of arctan(sqrt(x(1 - x))) dx. Hmm, let's start by understanding the problem. The integrand is arctan of the square root of x times (1 - x). That square root expression, sqrt(x(1 - x)), looks familiar. It's symmetric around x = 0.5 because if I substitute x with 1 - x, the expression remains the same. So maybe there's some symmetry I can exploit here.

First, let me write down the integral again to make sure I have it right:

∫₀¹ arctan(√(x(1 - x))) dx

I wonder if substitution would help here. Let me consider substitution to simplify the square root term. Let’s set t = x - 0.5, which might center the integral around zero. But I'm not sure if that helps. Alternatively, maybe a trigonometric substitution. The expression x(1 - x) is similar to the form of a quadratic that can be rewritten as (1/4) - (x - 1/2)^2. Let me check that:

x(1 - x) = x - x² = -x² + x = -(x² - x) = -(x² - x + 1/4 - 1/4) = -( (x - 1/2)^2 - 1/4 ) = - (x - 1/2)^2 + 1/4

So, x(1 - x) = 1/4 - (x - 1/2)^2. Therefore, sqrt(x(1 - x)) = sqrt(1/4 - (x - 1/2)^2). That looks like the equation of a semicircle with radius 1/2 centered at (1/2, 0). So integrating over this from 0 to 1 is like integrating over the top half of a circle. But how does that help with the arctan?

Alternatively, maybe substitution u = x - 1/2, but I'm not sure. Let's think about integrating arctan of a function. Integration by parts might be useful here. Remember that the integral of arctan(u) can sometimes be handled by parts, letting u = arctan(...) and dv = dx. Let me try that.

Let’s set:

Let u = arctan(√(x(1 - x))) => du/dx = [1 / (1 + x(1 - x))] * ( derivative of sqrt(x(1 - x)) )

Then dv = dx => v = x

But integration by parts formula is ∫u dv = uv - ∫v du. Let's compute du first.

First, derivative of sqrt(x(1 - x)) is (1/(2 sqrt(x(1 - x)))) * (1 - 2x). So:

du/dx = [1 / (1 + x(1 - x))] * (1 - 2x)/(2 sqrt(x(1 - x)))

Therefore, du = [ (1 - 2x) / (2 sqrt(x(1 - x)) (1 + x(1 - x)) ) ] dx

So, integrating by parts:

uv - ∫v du = [x arctan(sqrt(x(1 - x)))] from 0 to 1 - ∫₀¹ x * [ (1 - 2x) / (2 sqrt(x(1 - x)) (1 + x(1 - x)) ) ] dx

Now, evaluating the boundary term [x arctan(...)] from 0 to 1. At x=1, sqrt(1*(1-1))=0, so arctan(0)=0. Similarly at x=0, same result. So the boundary term is 0 - 0 = 0. So the integral reduces to:

- ∫₀¹ x * (1 - 2x) / [ 2 sqrt(x(1 - x)) (1 + x(1 - x)) ] dx

Hmm, that seems complicated. Let me simplify the integrand. Let's write the integral as:

-1/2 ∫₀¹ [x(1 - 2x)] / [ sqrt(x(1 - x)) (1 + x(1 - x)) ] dx

Wait, but x(1 - 2x) over sqrt(x(1 - x))... Let me factor x in the numerator and denominator. Let's see:

x(1 - 2x) / sqrt(x(1 - x)) = x^{1} (1 - 2x) / [x^{1/2} (1 - x)^{1/2}] = x^{1 - 1/2} (1 - 2x) / (1 - x)^{1/2} = x^{1/2} (1 - 2x) / (1 - x)^{1/2}

So the integral becomes:

-1/2 ∫₀¹ [x^{1/2} (1 - 2x) / (1 - x)^{1/2} ] / (1 + x(1 - x)) dx

Hmm, this is getting messy. Maybe there's a substitution here. Let me consider substituting t = sqrt(x/(1 - x)). Let's try that. Let t = sqrt(x/(1 - x)). Then t² = x/(1 - x) => x = t²(1 - x) => x = t² - t² x => x(1 + t²) = t² => x = t² / (1 + t²). Then 1 - x = 1 - t²/(1 + t²) = (1 + t² - t²)/(1 + t²) = 1/(1 + t²). So dx/dt = [2t(1 + t²) - t²*2t]/(1 + t²)^2 = [2t + 2t³ - 2t³]/(1 + t²)^2 = 2t/(1 + t²)^2.

So dx = 2t/(1 + t²)^2 dt.

Now, let's see what the integrand becomes. Let's substitute x = t²/(1 + t²). Then sqrt(x(1 - x)) = sqrt( t²/(1 + t²) * 1/(1 + t²) ) = sqrt( t²/(1 + t²)^2 ) = t/(1 + t²).

So the original integrand was arctan(sqrt(x(1 - x))) = arctan(t/(1 + t²)). Wait, but in the substitution, t is sqrt(x/(1 - x)), so when x goes from 0 to 1, t goes from 0 to infinity. Hmm, but maybe this substitution complicates things. Let me check.

Wait, perhaps another substitution. Let me think. Alternatively, maybe use substitution based on the symmetry. Since the original integrand is symmetric around x = 0.5, maybe substitute x = 1 - t. Let’s try that. Let x = 1 - t, then when x=0, t=1; x=1, t=0. The integral becomes ∫₁⁰ arctan(sqrt((1 - t)t)) (-dt) = ∫₀¹ arctan(sqrt(t(1 - t))) dt. So the integral is equal to itself, which tells us that it's symmetric, but that might not help directly.

Alternatively, maybe use substitution x = sin²θ. Let's try that. Let x = sin²θ, so dx = 2 sinθ cosθ dθ. Then sqrt(x(1 - x)) = sqrt(sin²θ cos²θ) = sinθ cosθ. So arctan(sinθ cosθ). The limits when x=0, θ=0; x=1, θ=π/2. So the integral becomes ∫₀^{π/2} arctan(sinθ cosθ) * 2 sinθ cosθ dθ.

Hmm, that might be a way to proceed. Let me write that:

I = ∫₀¹ arctan(√(x(1 - x))) dx = ∫₀^{π/2} arctan(sinθ cosθ) * 2 sinθ cosθ dθ

Let’s denote φ = θ, so:

I = 2 ∫₀^{π/2} arctan( (sinφ cosφ) ) sinφ cosφ dφ

But sinφ cosφ = (1/2) sin(2φ), so:

I = 2 ∫₀^{π/2} arctan( (1/2) sin(2φ) ) * (1/2) sin(2φ) dφ

Wait, because sinφ cosφ = (1/2) sin(2φ), so substituting:

I = 2 * (1/2) ∫₀^{π/2} arctan( (1/2) sin(2φ) ) sin(2φ) dφ = ∫₀^{π/2} arctan( (1/2) sin(2φ) ) sin(2φ) dφ

Now, let’s make substitution t = 2φ. When φ=0, t=0; φ=π/2, t=π. Then dφ = dt/2. So:

I = ∫₀^{π} arctan( (1/2) sin t ) sin t * (dt/2) = (1/2) ∫₀^{π} arctan( (1/2) sin t ) sin t dt

Hmm, not sure if that helps. Alternatively, maybe use series expansion for arctan. The arctan(z) can be expressed as a power series: arctan(z) = ∑_{n=0}^∞ (-1)^n z^{2n+1}/(2n+1) for |z| ≤ 1. But here z = (1/2) sin t, which is ≤ 1/2, so converges. Let's try that.

So, arctan( (1/2) sin t ) = ∑_{n=0}^∞ (-1)^n [ (1/2 sin t )^{2n+1} ] / (2n +1 )

Therefore, the integral becomes:

I = (1/2) ∫₀^{π} [ ∑_{n=0}^∞ (-1)^n (1/2)^{2n+1} sin^{2n+1} t / (2n +1) ] sin t dt

= (1/2) ∑_{n=0}^∞ [ (-1)^n (1/2)^{2n+1} / (2n +1) ] ∫₀^{π} sin^{2n+2} t dt

But integrating sin^{2n+2} t from 0 to π. The integral of sin^k t from 0 to π is 2 ∫₀^{π/2} sin^k t dt, and that is 2 * (sqrt(π) Γ((k+1)/2) ) / (2 Γ( (k/2) +1 )) )

But maybe there's a formula for that. The integral ∫₀^{π} sin^{m} t dt = 2 ∫₀^{π/2} sin^{m} t dt = 2 * (sqrt(π) Γ( (m+1)/2 ) ) / ( 2 Γ( m/2 +1 ) ) )

Alternatively, using the beta function: ∫₀^{π} sin^{m} t dt = 2 ∫₀^{π/2} sin^{m} t dt = 2 * (B(1/2, (m+1)/2 ) / 2 ) = B(1/2, (m+1)/2 )

But B(a,b) = Γ(a)Γ(b)/Γ(a+b). So:

∫₀^{π} sin^{m} t dt = Γ(1/2) Γ( (m+1)/2 ) / Γ( (m/2 ) +1 )

But Γ(1/2) = sqrt(π). So:

= sqrt(π) Γ( (m+1)/2 ) / Γ( (m/2 ) +1 )

So for m = 2n +2:

∫₀^{π} sin^{2n+2} t dt = sqrt(π) Γ( (2n +3)/2 ) / Γ( (2n +4)/2 / 2 )? Wait, no. Wait, m = 2n +2, so:

Γ( (m+1)/2 ) = Γ( (2n +3)/2 )

Γ( (m/2 ) +1 ) = Γ( (n +1 ) +1 ) = Γ(n +2 )

But Γ(n +2 ) = (n +1 )!

So the integral becomes sqrt(π) Γ( (2n +3)/2 ) / ( (n +1 )! )

But Γ( (2n +3)/2 ) can be expressed using the double factorial or other identities. For example, Γ(k + 1/2 ) = (sqrt(π)/2^k) (2k)! ) / k! )

Wait, more precisely, for integer k ≥0,

Γ(k + 1/2 ) = (sqrt(π)) (2k)! ) / (4^k k! )

Similarly, Γ( (2n +3)/2 ) = Γ( n + 3/2 ) = sqrt(π) (2n +2)! ) / (4^{n +1} (n +1)! ) )

Wait, let's check for k = n +1:

Γ( (n +1) + 1/2 ) = Γ( n + 3/2 ) = sqrt(π) (2n +2)! ) / (4^{n +1} (n +1)! ) )

Wait, maybe not exactly. Let me recall that:

Γ(n + 1/2 ) = (2n)! ) sqrt(π) / (4^n n! )

So for Γ(n + 3/2 ) = Γ( (n +1 ) + 1/2 ) = (2(n +1) )! sqrt(π) / (4^{n +1} (n +1)! ) )

Yes, that's correct. So:

Γ(n + 3/2 ) = sqrt(π) (2n +2)! ) / (4^{n +1} (n +1)! ) )

Therefore, the integral ∫₀^{π} sin^{2n +2} t dt = sqrt(π) * [ sqrt(π) (2n +2)! / (4^{n +1} (n +1)! ) ) ] / ( (n +1)! )

Wait, let me substitute back into the expression:

sqrt(π) * Γ( (2n +3)/2 ) / Γ( n +2 )

= sqrt(π) * [ sqrt(π) (2n +2)! / (4^{n +1} (n +1)! ) ) ] / ( (n +1)! )

= π (2n +2)! / (4^{n +1} (n +1)! )^2 )

Simplify:

(2n +2)! = (2n +2)(2n +1)! = 2(n +1)(2n +1)! )

But maybe it's better to write (2n +2)! = 2^{n +1} (n +1)! ) product_{k=1}^{n +1} (2k -1 )

Wait, alternatively, (2n +2)! = (2n +2)(2n +1)(2n)! )

But perhaps not helpful. Let's see:

So the integral becomes:

π (2n +2)! / (4^{n +1} (n +1)! )^2 )

But 4^{n +1} = 2^{2n +2}, and (2n +2)! = (2n +2)(2n +1)! )

Alternatively, let's write (2n +2)! = (2n +2)(2n +1)(2n)! )

But maybe we can express this in terms of binomial coefficients. Alternatively, note that (2n +2)! / ( (n +1)! )^2 ) is the central binomial coefficient for 2n +2 choose n +1, but scaled. Wait, the central binomial coefficient is (2n choose n ), so maybe not exactly.

Alternatively, let's note that (2n +2)! / ( (n +1)! )^2 ) = (2n +2)(2n +1)(2n)! ) / ( (n +1)! )^2 )

But (2n +2) = 2(n +1), so:

= 2(n +1)(2n +1)(2n)! ) / ( (n +1)! )^2 )

= 2(2n +1) (2n)! ) / ( (n +1)! ) (n! ) )

But (2n)! / (n! )^2 ) is the central binomial coefficient C(2n, n). So:

= 2(2n +1) C(2n, n) / (n +1 )

But C(2n, n) / (n +1 ) is the nth Catalan number. Hmm, not sure if that helps.

Alternatively, perhaps we can write this as:

(2n +2)! / ( (n +1)! )^2 ) = (2n +2)(2n +1) / ( (n +1)^2 ) * (2n)! / ( (n! )^2 )

= 2(2n +1)/(n +1) * C(2n, n )

But maybe this is not helpful. Let's just keep it as π (2n +2)! / (4^{n +1} (n +1)! )^2 )

So putting this back into the expression for I:

I = (1/2) ∑_{n=0}^∞ [ (-1)^n (1/2)^{2n+1} / (2n +1) ] * [ π (2n +2)! / (4^{n +1} (n +1)! )^2 ) ]

Simplify the terms:

First, (1/2)^{2n +1} = 1/2 * (1/4)^n

Then, 4^{n +1} = 4 *4^n

So:

I = (1/2) * ∑_{n=0}^∞ [ (-1)^n (1/2) (1/4)^n / (2n +1) ) ] * [ π (2n +2)! / (4 *4^n (n +1)! )^2 ) ]

Wait, let's compute the constants:

(1/2) * (1/2) * (1/4)^n * π / (4 *4^n ) = (1/4) * π /4 * (1/4)^{2n} ) = π/(16) * (1/16)^n )

Wait, no. Let me step back.

First, the coefficient from the series term:

[ (-1)^n (1/2)^{2n+1} / (2n +1) ] = [ (-1)^n (1/2) (1/4)^n / (2n +1) ]

The integral term is [ π (2n +2)! / (4^{n +1} (n +1)! )^2 ) ]

So combining the constants:

(1/2) * [ (1/2) (1/4)^n / (2n +1) ] * [ π (2n +2)! / (4^{n +1} (n +1)! )^2 ) ]

= (1/2) * (1/2) * π /4^{n +1} * (1/4)^n * (2n +2)! / [ (2n +1) (n +1)! )^2 ]

Wait, 4^{n +1} is 4*4^n, and (1/4)^n * 1/4^{n +1} = 1/(4^{2n +1} )

Wait, no:

Wait, the term from the series is (1/2)^{2n +1} = (1/2) * (1/4)^n

The term from the integral is 1/4^{n +1}

So multiplying these gives (1/2) * (1/4)^n * 1/4^{n +1} = (1/2) * 1/4^{2n +1} = 1/(2 *4^{2n +1}) = 1/(2 * 16^n *4) ) = 1/(8 *16^n )

Wait, 4^{2n +1} = (4^2)^n *4 = 16^n *4, so 1/4^{2n +1} = 1/(4 *16^n )

But let me check:

(1/4)^n * 1/4^{n +1} = 1/4^{2n +1}

Yes. So:

So overall, the coefficient becomes:

(1/2) * [ (-1)^n / (2n +1) ] * [ π (2n +2)! / ( (n +1)! )^2 ) ] * 1/4^{2n +1}

= π/2 * (-1)^n / (2n +1) * (2n +2)! / ( (n +1)! )^2 ) * 1/4^{2n +1}

Hmm, this seems very complicated. Maybe there's a better approach. Let me think again.

Alternatively, perhaps consider differentiating under the integral sign. Let’s define:

I(a) = ∫₀¹ arctan(a sqrt(x(1 - x))) dx

Then, compute I'(a) = ∫₀¹ [ d/da arctan(a sqrt(x(1 - x))) ] dx = ∫₀¹ [ sqrt(x(1 - x)) / (1 + a² x(1 - x)) ] dx

Then, integrating I'(a) from a=0 to a=1 would give I(1) - I(0). Since I(0) = ∫₀¹ arctan(0) dx = 0, so I(1) = ∫₀¹ I'(a) da

So, I = ∫₀¹ [ ∫₀¹ sqrt(x(1 - x)) / (1 + a² x(1 - x)) dx ] da

Maybe switch the order of integration:

I = ∫₀¹ sqrt(x(1 - x)) [ ∫₀¹ 1 / (1 + a² x(1 - x)) da ] dx

Compute the inner integral over a:

∫₀¹ 1 / (1 + a² x(1 - x)) da

Let’s set b = a sqrt(x(1 - x)), then da = db / sqrt(x(1 - x))

But limits when a=0, b=0; a=1, b=sqrt(x(1 - x))

So the integral becomes:

∫₀^{sqrt(x(1 - x))} 1 / (1 + b² ) * db / sqrt(x(1 - x)) )

= [1 / sqrt(x(1 - x)) ] arctan(b) from 0 to sqrt(x(1 - x)) )

= [1 / sqrt(x(1 - x)) ] arctan( sqrt(x(1 - x)) )

Therefore, the inner integral is arctan( sqrt(x(1 - x)) ) / sqrt(x(1 - x))

Therefore, I = ∫₀¹ sqrt(x(1 - x)) * [ arctan( sqrt(x(1 - x)) ) / sqrt(x(1 - x)) ] dx = ∫₀¹ arctan( sqrt(x(1 - x)) ) dx

Wait, but that's the original integral. So this approach leads back to the original problem. So differentiating under the integral sign didn't help here. Hmm.

Alternative idea: Let’s consider substitution y = sqrt(x(1 - x)). Let’s see if we can express x in terms of y. But solving y = sqrt(x(1 - x)) gives y² = x - x² => x² -x + y² =0. The solutions are x = [1 ± sqrt(1 -4y²)] /2. But integrating over x from 0 to1, y ranges from 0 to 0.5 (since maximum of x(1 -x) is at x=0.5, which is 0.25, so sqrt(0.25)=0.5). So y goes from 0 to 0.5. But expressing x in terms of y would involve two branches, which complicates the substitution.

Alternatively, use substitution t = 2x -1, which centers the integral around 0. Let t = 2x -1, so x = (t +1)/2, dx = dt/2. Then when x=0, t=-1; x=1, t=1. The integral becomes:

∫_{-1}^{1} arctan( sqrt( ( (t +1)/2 )(1 - (t +1)/2 )) ) * (dt/2 )

Simplify the expression inside sqrt:

( (t +1)/2 )( (1 - t)/2 ) = (1 - t²)/4. So sqrt( (1 - t²)/4 ) = sqrt(1 - t²)/2. So the integral becomes:

(1/2) ∫_{-1}^{1} arctan( sqrt(1 - t²)/2 ) dt

Since the integrand is even (sqrt(1 - t²) is even), we can write:

(1/2)*2 ∫₀¹ arctan( sqrt(1 - t²)/2 ) dt = ∫₀¹ arctan( sqrt(1 - t²)/2 ) dt

Hmm, not sure if that helps. Maybe another substitution here. Let’s set u = sqrt(1 - t²)/2. Then t = sqrt(1 - (2u)^2 ). But this might not help.

Alternatively, use substitution t = sinθ. Let t = sinθ, then dt = cosθ dθ, and sqrt(1 - t²) = cosθ. The integral becomes:

∫₀^{π/2} arctan( cosθ / 2 ) cosθ dθ

Wait, no. Wait, t ranges from 0 to1, so θ ranges from 0 to π/2. So:

∫₀¹ arctan( sqrt(1 - t²)/2 ) dt = ∫₀^{π/2} arctan( (cosθ)/2 ) cosθ dθ

Hmm, maybe this is easier. Let me write this as:

I = ∫₀^{π/2} arctan( (cosθ)/2 ) cosθ dθ

Hmm, perhaps integrate by parts here. Let’s set u = arctan( (cosθ)/2 ), dv = cosθ dθ. Then du/dθ = [1 / (1 + (cos²θ)/4 ) ] * (-sinθ)/2, and v = sinθ.

So integration by parts gives:

uv |₀^{π/2} - ∫₀^{π/2} v du

At θ=π/2, cosθ=0, so arctan(0)=0, so uv term at π/2 is 0. At θ=0, sinθ=0, so uv term is 0. So the integral becomes:

- ∫₀^{π/2} sinθ * [ - sinθ / (2 (1 + (cos²θ)/4 ) ) ] dθ

= (1/2) ∫₀^{π/2} [ sin²θ / (1 + (cos²θ)/4 ) ] dθ

Simplify denominator: 1 + (cos²θ)/4 = (4 + cos²θ)/4. So:

= (1/2) ∫₀^{π/2} [ sin²θ *4 / (4 + cos²θ) ] dθ = 2 ∫₀^{π/2} [ sin²θ / (4 + cos²θ) ] dθ

Hmm, this seems more manageable. Let's write sin²θ = 1 - cos²θ:

= 2 ∫₀^{π/2} [ (1 - cos²θ) / (4 + cos²θ) ] dθ

= 2 ∫₀^{π/2} [ (4 + cos²θ - 5 ) / (4 + cos²θ) ] dθ

= 2 ∫₀^{π/2} [1 - 5/(4 + cos²θ) ] dθ

= 2 [ ∫₀^{π/2} dθ -5 ∫₀^{π/2} 1/(4 + cos²θ) dθ ]

Compute the first integral: ∫₀^{π/2} dθ = π/2

The second integral: ∫₀^{π/2} 1/(4 + cos²θ) dθ

To compute this, we can use the standard integral ∫ dx/(a + b cos²x ). The formula is:

∫ dx/(a + b cos²x ) = (1/sqrt(a(a + b))) ) arctan( sqrt( (a + b)/a ) tanx ) + C

For our case, a=4, b=1. So:

∫ dx/(4 + cos²x ) = (1/sqrt(4*5)) arctan( sqrt(5/4) tanx ) + C = (1/(2 sqrt(5))) arctan( (sqrt(5)/2) tanx ) + C

Evaluating from 0 to π/2:

At π/2, tanx approaches infinity, so arctan( (sqrt(5)/2) * infinity ) = arctan(∞) = π/2

At 0, tanx=0, so arctan(0)=0

Therefore, the integral is (1/(2 sqrt(5))) [ π/2 - 0 ] = π/(4 sqrt(5))

Therefore, the second integral is π/(4 sqrt(5))

Putting back into the expression for I:

I = 2 [ π/2 -5 * π/(4 sqrt(5)) ] = 2*( π/2 - (5π)/(4 sqrt(5)) )

Simplify:

= π - (5π)/(2 sqrt(5)) = π - (5π)/(2 sqrt(5)) * (sqrt(5)/sqrt(5)) = π - (5π sqrt(5))/(10) = π - (π sqrt(5))/2

Wait, let's check:

5/(4 sqrt(5)) = (5)/(4 sqrt(5)) = sqrt(5)/4

Because 5/sqrt(5) = sqrt(5). So 5/(4 sqrt(5)) = sqrt(5)/4. Therefore:

I = 2 [ π/2 -5 * π/(4 sqrt(5)) ] = 2*( π/2 - π sqrt(5)/4 ) = 2*( (2π - π sqrt(5))/4 ) = (2π - π sqrt(5))/2 = π(2 - sqrt(5))/2

Wait, let me verify:

Wait, 5/(4 sqrt(5)) = (sqrt(5))^2/(4 sqrt(5)) )= sqrt(5)/4. So yes, 5/(4 sqrt(5)) = sqrt(5)/4.

So:

I = 2*( π/2 - π sqrt(5)/4 ) = π - π sqrt(5)/2 = π(1 - sqrt(5)/2 )

But wait, this is the result of the integral after substitution. Wait, let's recap:

We had I = ∫₀¹ arctan( sqrt(x(1 - x)) ) dx = ∫₀^{π/2} arctan( (cosθ)/2 ) cosθ dθ

Then after integration by parts, we arrived at:

I = 2 [ π/2 -5 * π/(4 sqrt(5)) ] = π - (5π)/(2 sqrt(5)) = π - (π sqrt(5))/2

But this seems to give a negative result, which can't be right since the integral of a positive function should be positive. Wait, sqrt(5) is approximately 2.236, so sqrt(5)/2 ≈1.118, so 1 -1.118 ≈ -0.118, which would make I ≈ -0.118π, which is negative. But the integral is of a positive function, so this can't be correct. Therefore, there must be a mistake in the calculation.

Let me check the steps might have gone wrong.

Starting from:

I = ∫₀¹ arctan( sqrt(x(1 - x)) ) dx

We used substitution t = 2x -1, leading to:

I = ∫₀¹ arctan( sqrt(1 - t²)/2 ) dt

Then substitution t = sinθ, leading to:

I = ∫₀^{π/2} arctan( (cosθ)/2 ) cosθ dθ

Then integration by parts:

u = arctan( (cosθ)/2 ), dv = cosθ dθ

du/dθ = [1 / (1 + (cos²θ)/4 ) ] * (-sinθ)/2

v = sinθ

Then the integral became:

- ∫₀^{π/2} sinθ * [ - sinθ / (2 (1 + (cos²θ)/4 ) ) ] dθ

= (1/2) ∫₀^{π/2} [ sin²θ / (1 + (cos²θ)/4 ) ] dθ

Then we rewrote sin²θ = 1 - cos²θ:

= (1/2) ∫₀^{π/2} [ (1 - cos²θ) / (1 + (cos²θ)/4 ) ] dθ

Wait, but denominator is 1 + (cos²θ)/4, not 4 + cos²θ. So when we rewrote the denominator as (4 + cos²θ)/4, that's incorrect. Wait, 1 + (cos²θ)/4 = (4 + cos²θ)/4. Yes, that's correct. So then:

= (1/2) ∫₀^{π/2} [ (1 - cos²θ) *4 / (4 + cos²θ) ] dθ = 2 ∫₀^{π/2} [ (1 - cos²θ) / (4 + cos²θ) ] dθ

Then, split into:

= 2 ∫₀^{π/2} [ (4 + cos²θ -5 ) / (4 + cos²θ) ] dθ

Wait, 1 - cos²θ = (4 + cos²θ -5 )? Let's check:

4 + cos²θ -5 = cos²θ -1 = -(1 - cos²θ) = -sin²θ. So this step is incorrect. That's the mistake.

Ah, yes! That's wrong. The correct way to split:

We have:

(1 - cos²θ) / (4 + cos²θ) = [ (4 + cos²θ) - (4 + cos²θ + cos²θ -1 ) ] / (4 + cos²θ). Wait, no. Let me think.

Wait, the numerator is 1 - cos²θ, and the denominator is 4 + cos²θ. To split this, perhaps express as:

= [ (4 + cos²θ) - (4 + cos²θ + cos²θ -1 ) ] / (4 + cos²θ). Hmm, not helpful.

Alternatively, perhaps write:

1 - cos²θ = (4 + cos²θ) - (3 + 2 cos²θ )

But that also doesn't help. Alternatively, maybe split as:

(1 - cos²θ)/(4 + cos²θ) = [A(4 + cos²θ) + B]/(4 + cos²θ). But this might not be useful.

Alternatively, note that:

(1 - cos²θ)/(4 + cos²θ) = [ (4 + cos²θ) - (3 + 2 cos²θ) ] / (4 + cos²θ) = 1 - (3 + 2 cos²θ)/(4 + cos²θ)

But not sure. Alternatively, use substitution.

Let’s set u = cosθ, then du = -sinθ dθ. But the integral is from θ=0 to π/2, so u from 1 to 0. Let's try:

∫ [ (1 - u²) / (4 + u²) ] (-du/sqrt(1 - u²)) )

But this seems complicated. Alternatively, use substitution t = tanθ. Let’s try that.

Let t = tanθ, then θ from 0 to π/2 corresponds to t from 0 to ∞. Then cosθ = 1/sqrt(1 + t²), dθ = dt/(1 + t²)

So the integral becomes:

2 ∫₀^{∞} [ (1 - (1/(1 + t²)) ) / (4 + (1/(1 + t²)) ) ] * (dt/(1 + t²))

Simplify numerator:

1 - 1/(1 + t²) = t²/(1 + t²)

Denominator:

4 + 1/(1 + t²) = (4(1 + t²) +1 ) / (1 + t²) = (4 +4 t² +1 ) / (1 + t²) = (5 +4 t² ) / (1 + t²)

So the integral becomes:

2 ∫₀^{∞} [ t²/(1 + t²) ) / ( (5 +4 t² ) / (1 + t²) ) ] * dt/(1 + t² )

= 2 ∫₀^{∞} [ t² / (5 +4 t² ) ] * dt/(1 + t² )

= 2 ∫₀^{∞} t² / [ (5 +4 t²)(1 + t²) ] dt

This is a rational function, so we can use partial fractions. Let’s decompose:

t² / [ (5 +4 t²)(1 + t²) ] = A/(1 + t²) + B/(5 +4 t²)

Multiply both sides by (5 +4 t²)(1 + t²):

t² = A(5 +4 t²) + B(1 + t²)

Expand:

t² = 5A +4A t² + B + B t²

Group terms:

t² = (4A + B) t² + (5A + B)

Equate coefficients:

For t²: 1 =4A + B

For constant term: 0 =5A + B

Solve the system:

From the second equation: B = -5A

Substitute into first equation: 1 =4A -5A = -A => A = -1

Then B = -5*(-1) =5

So decomposition is:

t² / [ (5 +4 t²)(1 + t²) ] = -1/(1 + t²) +5/(5 +4 t²)

Therefore, the integral becomes:

2 ∫₀^{∞} [ -1/(1 + t²) +5/(5 +4 t²) ] dt

= 2 [ - ∫₀^{∞} 1/(1 + t²) dt +5 ∫₀^{∞} 1/(5 +4 t²) dt ]

Compute each integral:

First integral: ∫₀^{∞} 1/(1 + t²) dt = π/2

Second integral: ∫₀^{∞} 1/(5 +4 t²) dt. Let’s substitute u = (2 t)/sqrt(5), so t = (sqrt(5)/2) u, dt = sqrt(5)/2 du. Then:

∫₀^{∞} 1/(5 +4 t²) dt = ∫₀^{∞} 1/(5 +5 u² ) * (sqrt(5)/2) du = (sqrt(5)/2) ∫₀^{∞} 1/(5(1 + u²)) du = (sqrt(5)/10) * π/2 = π sqrt(5)/20

Therefore, the integral becomes:

2 [ -π/2 +5*(π sqrt(5)/20 ) ] = 2 [ -π/2 + π sqrt(5)/4 ] = 2*(-π/2) + 2*(π sqrt(5)/4 ) = -π + π sqrt(5)/2

So I = -π + (π sqrt(5))/2? Wait, no. Wait, the integral we computed was the expression for I after substitution, which was:

I = ∫₀¹ arctan( sqrt(x(1 - x)) ) dx = -π + (π sqrt(5))/2

Wait, but this gives I = π( sqrt(5)/2 -1 )

But sqrt(5)/2 is approximately 1.118, so sqrt(5)/2 -1 ≈0.118, so I ≈0.118π ≈0.371, which is positive. That makes sense.

So the exact value is π( sqrt(5)/2 -1 )

But let's check the steps again to ensure no mistakes.

We had:

I = ∫₀¹ arctan( sqrt(x(1 - x)) ) dx

After substitution and integration by parts, we found:

I = -π + (π sqrt(5))/2

Wait, no. Wait, the final result was:

I = -π + (π sqrt(5))/2 = π( sqrt(5)/2 -1 )

Yes. So the exact answer is π( sqrt(5)/2 -1 )

But let's verify with numerical approximation. Let's compute sqrt(5) ≈2.23607, so sqrt(5)/2 ≈1.11803, subtract 1 gives 0.11803, multiplied by π≈3.14159 gives approximately 0.371.

Let me check with a numerical integral. For example, using a calculator or approximate integration.

Alternatively, compute the integral from 0 to1 of arctan(sqrt(x(1 -x))) dx numerically. Let's approximate it.

Using Simpson's rule with n=4 intervals:

But maybe better to use a calculator. Alternatively, use approximate value.

But since the exact answer is π( sqrt(5)/2 -1 ), which is approximately 3.14159*(1.11803/2 -1) = 3.14159*(0.559015 -1) = 3.14159*(-0.440985) which is negative. Wait, that can't be. Wait, no:

Wait, sqrt(5)/2 is approximately 2.23607/2=1.11803. Then sqrt(5)/2 -1 =0.11803. So π*0.11803≈0.371.

Yes, that's correct. So the exact answer is π( sqrt(5)/2 -1 )

But let's write it as π( (sqrt(5) -2)/2 )

Which is π( sqrt(5) -2 )/2

So, the exact answer is (π/2)(sqrt(5) -2 )

Now, the numerical approximation. Let's compute this:

sqrt(5) ≈2.2360679775

sqrt(5) -2 ≈0.2360679775

Multiply by π/2: 0.2360679775 * 1.5707963268 ≈0.2360679775 *1.5707963268

Calculate:

0.2 *1.5707963268 =0.31415926536

0.03 *1.5707963268=0.0471238898

0.006 *1.5707963268≈0.009424779

0.0000679775 *1.5707963268≈0.00010681

Adding up: 0.31415926536 +0.0471238898=0.36128315516 +0.009424779=0.37070793416 +0.00010681≈0.370814744

So approximately 0.370814744, which rounds to 0.3708147441 when rounded to 10 decimal places.

But let me verify with a more precise computation.

Alternatively, use calculator:

Compute (sqrt(5) -2)/2 * π:

sqrt(5) =2.2360679774997898

sqrt(5) -2=0.2360679774997898

Divide by 2:0.1180339887498949

Multiply by π:0.1180339887498949 *3.141592653589793=0.37081647204

So approximately 0.3708164720, which rounds to 0.3708164720 when rounded to 10 decimal places.

But let me check with numerical integration. Let's approximate the integral numerically.

The integral from 0 to1 of arctan(sqrt(x(1 -x))) dx.

Using substitution x = sin^2θ, as before, the integral becomes:

2 ∫₀^{π/2} arctan(sinθ cosθ) sinθ cosθ dθ

But perhaps using numerical methods.

Alternatively, use a calculator or computational tool. But since I don't have one here, I can use the exact expression we derived: π( sqrt(5)/2 -1 ) ≈0.37081647204.

So the exact answer is (π/2)(sqrt(5) -2 ), and the numerical approximation is approximately 0.3708164720.

Therefore, the final answer is:

Exact: (π/2)(sqrt(5) -2 )

Numerical: approximately 0.3708164720

So the JSON output should be:

{"answer": "\\frac{\\pi}{2}(\\sqrt{5} - 2)", "numerical_answer": "0.3708164720"}
</think>

{"answer": "\\frac{\\pi}{2}(\\sqrt{5} - 2)", "numerical_answer": "0.3708164720"}