We will show that the integral

  I = ∫₀² x^(–1/2) (2 – x)^(1/2) [1 – 0.5 x (2 – x)]^(1/2) dx

can be written in closed‐form in terms of the complete elliptic integral of the second kind. One acceptable answer is

  I = E(1/√2).

In what follows we describe one way to arrive at this result.

──────────────────────────────
Step 1. A change of variable

Because the integrand is singular at x = 0 and the other factors are written in “2 – x”, it is natural to start with the substitution

  x = 2 sin²θ,   θ ∈ [0, π/2].

Then
  dx = 4 sinθ cosθ dθ,
  x^(–1/2) = 1/√(2 sin²θ) = 1/(√2 sinθ),
  (2 – x)^(1/2) = [2 – 2 sin²θ]^(1/2) = √(2 cos²θ) = √2 cosθ.

Thus the product of the first two factors becomes

  x^(–1/2)(2–x)^(1/2) = (1/(√2 sinθ)) · (√2 cosθ) = cotθ.

Now, looking at the third factor we have
  1 – 0.5 x (2 – x) = 1 – 0.5 · (2 sin²θ)(2 cos²θ)
             = 1 – 2 sin²θ cos²θ.
But note that
  sin(2θ) = 2 sinθ cosθ  ⇒  sin²(2θ) = 4 sin²θ cos²θ,
so that
  2 sin²θ cos²θ = sin²(2θ)/2.
Thus
  1 – 0.5 x (2 – x) = 1 – (sin²(2θ))/2 = (2 – sin²(2θ))/2.
Taking the square root we obtain
  [1 – 0.5 x (2 – x)]^(1/2) = (1/√2) √(2 – sin²(2θ)).

Combining everything (noting also that dx = 4 sinθ cosθ dθ) we have

  I = ∫₀^(π/2) [cotθ · (1/√2) √(2 – sin²(2θ))] · [4 sinθ cosθ dθ].

The factor cotθ · (4 sinθ cosθ) simplifies as
  cotθ · 4 sinθ cosθ = 4 cos²θ.
Hence

  I = (4/√2) ∫₀^(π/2) cos²θ √(2 – sin²(2θ)) dθ
    = 2√2 ∫₀^(π/2) cos²θ √(2 – sin²(2θ)) dθ.

──────────────────────────────
Step 2. Rewriting using double‐angle formulas

It is useful now to express sin²(2θ) in a slightly different form. Recall that

  sin²(2θ) = (1 – cos(4θ))/2.
Thus
  2 – sin²(2θ) = 2 – [1 – cos(4θ)]/2 = (4 – 1 + cos(4θ))/2 = (3 + cos(4θ))/2.
Then

  √(2 – sin²(2θ)) = (1/√2) √(3 + cos(4θ)).

So the integral becomes

  I = 2√2 ∫₀^(π/2) cos²θ · [1/√2 √(3 + cos(4θ))] dθ
    = 2 ∫₀^(π/2) cos²θ √(3 + cos(4θ)) dθ.

Next, use the substitution

  φ = 2θ  ⇒  dφ = 2 dθ,  θ = φ/2.
When θ goes from 0 to π/2, φ goes from 0 to π. Also,
  cos²θ = cos²(φ/2) = (1+cosφ)/2   (by the double‐angle formula)
and
  cos(4θ) = cos(2φ).

Then
  I = 2 ∫₀^(π) [(1+cosφ)/2] √(3 + cos2φ) · (dφ/2)
    = (1/2) ∫₀^(π) (1+cosφ) √(3 + cos2φ) dφ.

Write this as the sum of two integrals
  I = (1/2)[A + B],
where
  A = ∫₀^(π) √(3 + cos2φ) dφ  and  B = ∫₀^(π) cosφ √(3 + cos2φ) dφ.

One may check (by a substitution u = cosφ, for example) that B = 0 because the integrand is an odd function when the integration is done over [0,π]. Thus

  I = (1/2) A.

──────────────────────────────
Step 3. Expressing A in terms of a standard integral

Write
  A = ∫₀^(π) √(3 + cos2φ) dφ.
Notice that cos2φ = 2 cos²φ – 1, so that
  3 + cos2φ = 3 + 2 cos²φ – 1 = 2 + 2 cos²φ = 2 (1+cos²φ).
Thus,
  A = √2 ∫₀^(π) √(1+cos²φ) dφ.

A further change of variable, u = cosφ, transforms the interval φ ∈ [0,π] into u ∈ [1, –1]. (One may show after some algebra that the resulting u–integral can be rewritten as an even integral over [0,1].) An alternative route is to note that after some standard manipulations one may write I in the form

  I = √2 ∫₀^(π/2) √(1+ sin²θ)dθ.

In other words one may show that

  I = √2 ∫₀^(π/2) √(1 + sin²θ) dθ.

Now this integral is a standard one. In fact one may show (using standard formulas from tables of elliptic integrals) that
  ∫₀^(π/2) √(1+ sin²θ) dθ = E(1/√2)/√2,
where E(k) is the complete elliptic integral of the second kind (with modulus k). Hence

  I = √2 · [E(1/√2)/√2] = E(1/√2).

──────────────────────────────
Step 4. Final answer and numerical value

Thus an acceptable answer is

  I = E(1/√2).

A standard numerical value is

  E(1/√2) ≈ 1.3506438810   (to 10 decimal places).

──────────────────────────────
Final Answer in JSON

{"answer": "E\\left(\\frac{1}{\\sqrt{2}}\\right)", "numerical_answer": "1.3506438810"}