Let's evaluate:
\[
I = \int_0^1 x^{-1} \ln x \ln\left(\frac{2+x}{2-x}\right) dx
\]

## Step 1: Analytic Evaluation

### 1. Expand the logarithm
\[
\ln\left(\frac{2+x}{2-x}\right) = \ln(2+x) - \ln(2-x)
\]
So,
\[
I = \int_0^1 x^{-1} \ln x \left[\ln(2+x) - \ln(2-x)\right] dx = I_1 - I_2
\]
where
\[
I_1 = \int_0^1 x^{-1} \ln x \ln(2+x) dx
\]
\[
I_2 = \int_0^1 x^{-1} \ln x \ln(2-x) dx
\]

### 2. Series expansion for \(\ln(2+x)\) and \(\ln(2-x)\)

We use the Taylor series for \(\ln(2+x)\) at \(x=0\):
\[
\ln(2+x) = \ln 2 + \sum_{n=1}^\infty \frac{(-1)^{n+1}}{n 2^n} x^n
\]
Similarly,
\[
\ln(2-x) = \ln 2 - \sum_{n=1}^\infty \frac{1}{n 2^n} x^n
\]
So,
\[
\ln(2+x) - \ln(2-x) = \sum_{n=1}^\infty \frac{(-1)^{n+1} + 1}{n 2^n}x^n
\]
But notice that
\[
(-1)^{n+1} + 1 = \begin{cases}
0 & \text{if } n\text{ is odd} \\
2 & \text{if } n \text{ is even}
\end{cases}
\]
So the sum only ranges over even \(n\):
\[
\ln(2+x) - \ln(2-x) = 2\sum_{k=1}^\infty \frac{1}{2k 2^{2k}} x^{2k}
= \sum_{k=1}^\infty \frac{1}{k 4^k} x^{2k}
\]

Therefore,
\[
I = \int_0^1 x^{-1} \ln x \left( \sum_{k=1}^\infty \frac{1}{k 4^k} x^{2k} \right) dx
= \sum_{k=1}^\infty \frac{1}{k 4^k} \int_0^1 x^{-1} \ln x \cdot x^{2k} dx
\]
\[
= \sum_{k=1}^\infty \frac{1}{k 4^k} \int_0^1 x^{2k-1} \ln x dx
\]

Recall:
\[
\int_0^1 x^a \ln x dx = -\frac{1}{(a+1)^2}
\]

So with \(a = 2k-1\):
\[
I = \sum_{k=1}^\infty \frac{1}{k 4^k} \left(- \frac{1}{(2k)^2}\right)
= -\sum_{k=1}^\infty \frac{1}{k (2k)^2 4^k}
= -\sum_{k=1}^\infty \frac{1}{4k^3 4^k}
= -\sum_{k=1}^\infty \frac{1}{4^{k+1} k^3}
\]

Now,
\[
\sum_{k=1}^\infty \frac{1}{4^{k}k^3} = \mathrm{Li}_3\left(\frac{1}{4}\right)
\]
Thus,
\[
I = -\frac{1}{4} \sum_{k=1}^\infty \frac{1}{4^{k} k^3}
= -\frac{1}{4} \mathrm{Li}_3\left(\frac{1}{4}\right)
\]

## Step 2: Final Exact Answer

\[
\boxed{I = -\frac{1}{4} \mathrm{Li}_3\left(\frac{1}{4}\right)}
\]

## Step 3: Numerical Value

Compute \(\mathrm{Li}_3(1/4)\):

- \(\mathrm{Li}_3\left(\frac{1}{4}\right) \approx 0.2676531740\)

Thus,
- \(I \approx -\frac{1}{4} \times 0.2676531740 = -0.0669132935\)

## Step 4: JSON Output

```json
{"answer": "-\\frac{1}{4}\\operatorname{Li}_3\\left(\\frac{1}{4}\\right)", "numerical_answer": "-0.0669132935"}
```