

To solve the definite integral \(\int_0^\infty \frac{\{x\}^{\lceil x \rceil}}{1+\lceil x \rceil} \, dx\), we analyze the integrand over intervals where the ceiling function \(\lceil x \rceil\) and fractional part \(\{x\}\) are constant.

### Step 1: Break the integral into intervals
The ceiling function \(\lceil x \rceil\) is constant over intervals of the form \([n, n+1)\) for non-negative integers \(n\). The fractional part \(\{x\} = x - \lfloor x \rfloor\) simplifies to \(x - n\) on \([n, n+1)\).

### Step 2: Evaluate the integral over each interval
- **For \(n = 0\) (interval \([0, 1)\))**:  
  Here, \(\lceil x \rceil = 1\) for \(x \in (0, 1)\) (since \(x=0\) is a single point with measure zero), and \(\{x\} = x\). The integrand becomes \(\frac{x^1}{1+1} = \frac{x}{2}\).  
  The integral over \([0, 1)\) is:  
  \[
  \int_0^1 \frac{x}{2} \, dx = \frac{1}{2} \cdot \frac{x^2}{2} \bigg|_0^1 = \frac{1}{4}.
  \]

- **For \(n \geq 1\) (interval \([n, n+1)\))**:  
  Here, \(\lceil x \rceil = n+1\) for \(x \in (n, n+1)\) (since \(x=n\) is a single point), and \(\{x\} = x - n\). The integrand becomes \(\frac{(x - n)^{n+1}}{1 + (n+1)} = \frac{(x - n)^{n+1}}{n+2}\).  
  Substituting \(t = x - n\) (so \(t \in [0, 1)\)), the integral over \([n, n+1)\) becomes:  
  \[
  \int_n^{n+1} \frac{(x - n)^{n+1}}{n+2} \, dx = \int_0^1 \frac{t^{n+1}}{n+2} \, dt = \frac{1}{n+2} \cdot \frac{t^{n+2}}{n+2} \bigg|_0^1 = \frac{1}{(n+2)^2}.
  \]

### Step 3: Sum the results over all intervals
The total integral is the sum of the integral over \([0, 1)\) and the sum over \(n \geq 1\):  
\[
\int_0^\infty \frac{\{x\}^{\lceil x \rceil}}{1+\lceil x \rceil} \, dx = \frac{1}{4} + \sum_{n=1}^\infty \frac{1}{(n+2)^2}.
\]

### Step 4: Simplify the infinite sum
The sum \(\sum_{n=1}^\infty \frac{1}{(n+2)^2}\) is equivalent to \(\sum_{k=3}^\infty \frac{1}{k^2}\) (by substituting \(k = n+2\)). Using the known result for the Basel problem, \(\sum_{k=1}^\infty \frac{1}{k^2} = \frac{\pi^2}{6}\), we have:  
\[
\sum_{k=3}^\infty \frac{1}{k^2} = \frac{\pi^2}{6} - \frac{1}{1^2} - \frac{1}{2^2} = \frac{\pi^2}{6} - \frac{5}{4}.
\]

### Step 5: Combine terms
Adding the integral over \([0, 1)\) to the sum:  
\[
\int_0^\infty \frac{\{x\}^{\lceil x \rceil}}{1+\lceil x \rceil} \, dx = \frac{1}{4} + \left( \frac{\pi^2}{6} - \frac{5}{4} \right) = \frac{\pi^2}{6} - 1.
\]

### Numerical Approximation
Using \(\pi \approx 3.141592653589793\), we find \(\pi^2 \approx 9.869604401089358\). Thus:  
\[
\frac{\pi^2}{6} - 1 \approx \frac{9.869604401089358}{6} - 1 \approx 1.6449340668482263 - 1 = 0.6449340668482263.
\]

Rounded to 10 decimal places, the numerical approximation is \(0.6449340668\).

{"answer": "\(\frac{\pi^2}{6} - 1\)", "numerical_answer": "0.6449340668"}