We wish to evaluate

  I = ∫ from –1 to 1 of 1/(3^x + 1) dx.

Step 1. Define
  f(x) = 1/(3^x + 1).

Step 2. Consider f(–x). We compute:
  f(–x) = 1/(3^(–x) + 1) = 1/((1/3^x) + 1) = 1/((1 + 3^x)/3^x) = 3^x/(1 + 3^x).

Step 3. Add f(x) and f(–x):
  f(x) + f(–x) = 1/(3^x + 1) + 3^x/(3^x + 1) = (1 + 3^x)/(3^x + 1) = 1.

Step 4. Integrate over the interval [–1, 1]:
  ∫ from –1 to 1 f(x) dx + ∫ from –1 to 1 f(–x) dx = ∫ from –1 to 1 1 dx = 2.
But since the substitution x → –x in the second integral does not change the integration bounds and the integrals are effectively equal, we have:
  2 ∫ from –1 to 1 f(x) dx = 2,
which implies that
  ∫ from –1 to 1 f(x) dx = 1.

Step 5. Final answers:
The exact answer is 1. Its numerical approximation is 1.0000000000 (to 10 decimal places).

{"answer": "$1$", "numerical_answer": "1.0000000000"}