<think>
Okay, let's tackle this integral: ∫₀² x arcsin(0.5√(x(2−x))) dx. Hmm, first, I need to compute this analytically. The integrand is x times the inverse sine of a square root function. The limits are from 0 to 2. Let me see... Maybe a substitution would help here. The argument inside the arcsin is 0.5√(x(2−x)). Let me simplify that expression first.

So, 0.5√(x(2−x)) can be written as (1/2)√(2x - x²). Let me check if this resembles a known trigonometric identity. The expression under the square root is 2x - x², which can be rewritten as 1 - (x - 1)². Let me verify that: expanding (x - 1)² gives x² - 2x + 1, so 1 - (x - 1)² is 1 - x² + 2x -1 = 2x - x². Yes, that's correct. So, √(2x - x²) = √(1 - (x - 1)²). Therefore, the argument inside arcsin is (1/2)√(1 - (x - 1)²). Wait, but arcsin usually takes an argument that's a sine function. Maybe a substitution where (x - 1) = sinθ or something like that?

Alternatively, let's consider a substitution to simplify the integral. Let me set t = x - 1. Then, when x=0, t=-1; when x=2, t=1. The integral becomes ∫_{-1}^{1} (t + 1) arcsin(0.5√(1 - t²)) dt. Hmm, but the arcsin term now has √(1 - t²), which is similar to the sine of an angle. Let me think. If I set t = sinθ, then √(1 - t²) = cosθ. Then, arcsin(0.5 cosθ). Wait, but 0.5 cosθ is between -0.5 and 0.5. Hmm, maybe another substitution. Alternatively, perhaps a trigonometric substitution for the original variable x.

Alternatively, let's consider the expression inside arcsin: (1/2)√(x(2 - x)). Let me set this equal to sinθ. So, sinθ = (1/2)√(x(2 - x)). Then, θ = arcsin[(1/2)√(x(2 - x))]. Then, maybe we can express x in terms of θ. Let's square both sides: sin²θ = (1/4)x(2 - x). Multiply both sides by 4: 4 sin²θ = x(2 - x). Let's rearrange: x² - 2x + 4 sin²θ = 0. Wait, that's a quadratic in x. Solving for x: x = [2 ± √(4 - 16 sin²θ)] / 2. Hmm, this might complicate things. Maybe not the best approach.

Alternatively, let's consider a substitution for the entire integral. Let me try substitution u = x - 1, as before. Then, x = u + 1, dx = du. The integral becomes ∫_{-1}^{1 (u + 1) arcsin(0.5√{(u + 1)(1 - u)}) du. The expression inside the square root is (u + 1)(1 - u) = 1 - u². So, √(1 - u²). Therefore, the integrand becomes (u + 1) arcsin(0.5√(1 - u²)) du. Hmm, this seems a bit simpler. The function is now symmetric around u=0. Let's check if the integrand is even or odd. The term (u + 1) is not symmetric, but maybe we can split the integral into two parts: one with u and one with 1. So, ∫_{-1}^1 u arcsin(0.5√(1 - u²)) du + ∫_{-1}^1 arcsin(0.5√(1 - u²)) du. The first integral is an odd function integrated over symmetric limits, so it should be zero. Therefore, the integral reduces to ∫_{-1}^1 arcsin(0.5√(1 - u²)) du. Then, but we have to multiply by 2 because the original substitution was from x=0 to x=2, which became u=-1 to u=1. Wait, no, the substitution was x = u + 1, so the integral is already over u from -1 to 1. So, the original integral is equal to ∫_{-1}^1 (u + 1) arcsin(0.5√(1 - u²)) du. Then, as I said, the u term is odd, so integrating from -1 to 1 gives zero. Therefore, the integral simplifies to ∫_{-1}^1 arcsin(0.5√(1 - u²)) du. Wait, but the integrand here is arcsin(0.5√(1 - u²)). Let me check if this is an even function. Since √(1 - u²) is even, and arcsin is an odd function, but here the argument is 0.5 times an even function, so the argument is even. Then, arcsin of an even function is even, because arcsin(-y) = -arcsin(y), but if y is even, then arcsin(y(-u)) = arcsin(y(u)), so the whole integrand is even. Therefore, the integral from -1 to 1 is twice the integral from 0 to 1. So, the original integral becomes 2 * ∫₀¹ arcsin(0.5√(1 - u²)) du. Hmm, but this seems a bit more manageable. Let me denote this integral as I = 2 * ∫₀¹ arcsin(0.5√(1 - u²)) du. Now, how to compute this integral.

Alternatively, maybe another substitution. Let me set t = √(1 - u²). Then, t = √(1 - u²), so u = √(1 - t²). Then, but when u goes from 0 to 1, t goes from 1 to 0. Hmm, maybe not helpful. Alternatively, set θ such that 0.5√(1 - u²) = sinφ. Then, √(1 - u²) = 2 sinφ. Then, 1 - u² = 4 sin²φ. So, u² = 1 - 4 sin²φ. Then, u = √(1 - 4 sin²φ). Hmm, but differentiating this might complicate things. Alternatively, maybe trigonometric substitution. Let me try substituting u = sinθ. Then, du = cosθ dθ. Then, when u=0, θ=0; u=1, θ=π/2. Then, √(1 - u²) = cosθ. So, the integrand becomes arcsin(0.5 cosθ). So, the integral becomes ∫₀^{π/2} arcsin(0.5 cosθ) * cosθ dθ. Wait, but the substitution was u = sinθ, so du = cosθ dθ. Therefore, the integral I is 2 * ∫₀^{π/2} arcsin(0.5 cosθ) * cosθ dθ. Hmm, not sure if this helps. Maybe integration by parts here. Let me set v = arcsin(0.5 cosθ), dv/dθ = derivative of arcsin. The derivative of arcsin(z) is 1/√(1 - z²) * dz/dθ. Here, z = 0.5 cosθ, so dz/dθ = -0.5 sinθ. Therefore, dv/dθ = [1 / √(1 - (0.5 cosθ)^2)] * (-0.5 sinθ). Then, if we set u = cosθ, then du/dθ = -sinθ. Wait, but in integration by parts, we need to set parts. Let me try:

Let me denote the integral as ∫ arcsin(0.5 cosθ) * cosθ dθ. Let me set:

Let’s let v = arcsin(0.5 cosθ), and dw = cosθ dθ. Then, dv = [1 / √(1 - (0.5 cosθ)^2)] * (-0.5 sinθ) dθ, and w = sinθ. Then, integration by parts gives v*w - ∫ w dv. So:

arcsin(0.5 cosθ) * sinθ - ∫ sinθ * [ -0.5 sinθ / √(1 - 0.25 cos²θ) ] dθ

Simplify:

arcsin(0.5 cosθ) * sinθ + 0.5 ∫ [ sin²θ / √(1 - 0.25 cos²θ) ] dθ

Hmm, this seems more complicated. Maybe not the best approach. Let me think of another substitution. Alternatively, perhaps express arcsin(0.5 cosθ) in terms of another angle. Let me set 0.5 cosθ = sinφ. Then, φ = arcsin(0.5 cosθ). Then, sinφ = 0.5 cosθ. Then, cosθ = 2 sinφ. But cosθ is between 0 and 1 when θ is in [0, π/2], so 2 sinφ must be between 0 and 1. Therefore, sinφ is between 0 and 0.5, so φ is between 0 and π/6. Then, θ and φ are related by cosθ = 2 sinφ. Let me express θ in terms of φ. Then, θ = arccos(2 sinφ). Then, dθ/dφ = derivative of arccos(2 sinφ). Let's compute that:

dθ/dφ = - [1 / √(1 - (2 sinφ)^2)] * 2 cosφ

But wait, 2 sinφ must be ≤1, so sinφ ≤0.5, which is true since φ ∈ [0, π/6]. So, √(1 - 4 sin²φ) is real. Therefore, dθ/dφ = - [2 cosφ] / √(1 - 4 sin²φ)

But this seems complicated. However, maybe changing variables from θ to φ would help. Let's try substituting φ = arcsin(0.5 cosθ). Then, when θ=0, cosθ=1, so φ=arcsin(0.5*1)=arcsin(0.5)=π/6. When θ=π/2, cosθ=0, so φ=arcsin(0)=0. So, the limits of integration would change from θ=0 to θ=π/2, to φ=π/6 to φ=0. Therefore, reversing the limits:

∫_{φ=π/6}^{φ=0} ... dφ. Let's write the integral in terms of φ. The original integral is:

I = 2 * ∫₀^{π/2} arcsin(0.5 cosθ) * cosθ dθ

Expressed in terms of φ:

I = 2 * ∫_{π/6}^0 φ * cosθ * [dθ/dφ] dφ

But dθ/dφ is negative, so flipping the limits:

I = 2 * ∫₀^{π/6} φ * cosθ * (-dθ/dφ) dφ

But we need to express cosθ and dθ/dφ in terms of φ. From earlier, we have:

cosθ = 2 sinφ

And dθ/dφ = - [2 cosφ] / √(1 - 4 sin²φ)

Therefore, substituting:

I = 2 * ∫₀^{π/6} φ * (2 sinφ) * [2 cosφ / √(1 - 4 sin²φ)] dφ

Wait, because cosθ = 2 sinφ, and dθ/dφ is negative, but we flipped the limits, so the negative cancels. Therefore:

I = 2 * ∫₀^{π/6} φ * (2 sinφ) * [2 cosφ / √(1 - 4 sin²φ)] dφ

Simplify the constants:

2 * 2 * 2 = 8, so 8 ∫₀^{π/6} [ sinφ cosφ φ / √(1 - 4 sin²φ) ] dφ

Hmm, this seems even more complicated. Maybe this substitution isn't helpful. Let me think of another approach.

Alternatively, going back to the original integral: ∫₀² x arcsin(0.5√(x(2−x))) dx. Let me consider a substitution that simplifies the square root. Let me set t = x - 1, as before. Then, x = t + 1, dx = dt, limits from t=-1 to t=1. The integral becomes ∫_{-1}^1 (t + 1) arcsin(0.5√(1 - t²)) dt. As before, the t term is odd, so the integral reduces to ∫_{-1}^1 arcsin(0.5√(1 - t²)) dt. Which is 2 ∫₀¹ arcsin(0.5√(1 - t²)) dt. Let me denote this as 2I. Now, let me make a substitution in I. Let’s set t = sinθ, so θ from 0 to π/2. Then, √(1 - t²) = cosθ, dt = cosθ dθ. Then, I becomes ∫₀^{π/2} arcsin(0.5 cosθ) cosθ dθ. So, the original integral is 2I = 2 ∫₀^{π/2} arcsin(0.5 cosθ) cosθ dθ. Hmm, this seems familiar. Let me try integrating by parts here. Let’s set u = arcsin(0.5 cosθ), dv = cosθ dθ. Then, du = [1 / √(1 - (0.5 cosθ)^2)] * (-0.5 sinθ) dθ, and v = sinθ. Integration by parts gives uv|₀^{π/2} - ∫ v du. 

Calculating the boundary term: [arcsin(0.5 cosθ) sinθ] from 0 to π/2. At θ=π/2, cosθ=0, so arcsin(0) = 0, so term is 0. At θ=0, cosθ=1, so arcsin(0.5*1)=arcsin(0.5)=π/6, and sinθ=0. So, the boundary term is 0 - (π/6 * 0) = 0. Therefore, the integral becomes - ∫₀^{π/2} sinθ * [ -0.5 sinθ / √(1 - 0.25 cos²θ) ] dθ. Simplify: 0.5 ∫₀^{π/2} [ sin²θ / √(1 - 0.25 cos²θ) ] dθ. So, the original integral is 2I = 2 * 0.5 ∫₀^{π/2} [ sin²θ / √(1 - 0.25 cos²θ) ] dθ = ∫₀^{π/2} [ sin²θ / √(1 - 0.25 cos²θ) ] dθ. Hmm, this seems more manageable. Let me simplify the denominator: √(1 - 0.25 cos²θ) = √( (4 - cos²θ)/4 ) = √(4 - cos²θ)/2. Therefore, the integral becomes ∫₀^{π/2} [ sin²θ / ( √(4 - cos²θ)/2 ) ] dθ = 2 ∫₀^{π/2} [ sin²θ / √(4 - cos²θ) ] dθ. So, 2 ∫₀^{π/2} sin²θ / √(4 - cos²θ) dθ. Let me make a substitution here. Let’s set u = cosθ. Then, du = -sinθ dθ. When θ=0, u=1; θ=π/2, u=0. The integral becomes 2 ∫₁⁰ [ (1 - u²) / √(4 - u²) ] (-du) = 2 ∫₀¹ [ (1 - u²) / √(4 - u²) ] du. Simplify the integrand: (1 - u²)/√(4 - u²) = [ (4 - u²) - 3 ] / √(4 - u²) = √(4 - u²) - 3 / √(4 - u²). Therefore, the integral becomes 2 ∫₀¹ [ √(4 - u²) - 3 / √(4 - u²) ] du. Split the integral: 2 [ ∫₀¹ √(4 - u²) du - 3 ∫₀¹ 1/√(4 - u²) du ]. Let's compute these two separately.

First integral: ∫√(4 - u²) du. This is a standard integral. The integral of √(a² - u²) du is (u/2)√(a² - u²) + (a²/2) arcsin(u/a) + C. Here, a=2. So, ∫√(4 - u²) du from 0 to1 is [ (u/2)√(4 - u²) + (4/2) arcsin(u/2) ] from 0 to1. At u=1: (1/2)√(3) + 2 arcsin(1/2) = (√3)/2 + 2*(π/6) = (√3)/2 + π/3. At u=0: 0 + 2*0 = 0. So, the first integral is (√3)/2 + π/3.

Second integral: ∫1/√(4 - u²) du. This is arcsin(u/2) + C. Evaluated from 0 to1: arcsin(1/2) - arcsin(0) = π/6 - 0 = π/6.

Putting it all together: 2 [ ( (√3)/2 + π/3 ) - 3*(π/6) ] = 2 [ (√3/2 + π/3 - π/2) ] = 2 [ √3/2 - π/6 ] = √3 - π/3.

Wait, the original integral was 2I, which we transformed into this expression. So, the result is √3 - π/3. Therefore, the value of the definite integral is √3 - π/3. Let me check the steps again to make sure.

Starting from the original integral, substitution t = x -1, then splitting into even and odd functions, leading to 2I where I is ∫₀¹ arcsin(0.5√(1 - t²)) dt. Then substitution t = sinθ, leading to integrating by parts, which after some steps led to the integral becoming √3 - π/3. Let me verify the numerical value. √3 is approximately 1.732, π/3 is approximately 1.047, so √3 - π/3 ≈ 0.685. Let me check with a quick numerical integration. If I plug in x=0 to 2, integrating x arcsin(0.5√(x(2−x))) dx. Let me approximate numerically. For example, at x=1, the argument inside arcsin is 0.5√(1*1)=0.5, so arcsin(0.5)=π/6≈0.523. So the integrand at x=1 is 1*(π/6)≈0.523. The function is likely to be around that value in the middle. The integral is approximately 0.685, which seems plausible. Let me compute √3 - π/3 numerically: √3≈1.7320508075688772, π≈3.141592653589793, so π/3≈1.0471975511965976. Then, 1.7320508075688772 - 1.0471975511965976 ≈ 0.6848532563722796. Rounded to 10 decimal places, that's approximately 0.6848532564. Let me check with another approach. Maybe using substitution from the beginning. Let me consider the original integral ∫₀² x arcsin(0.5√(x(2−x))) dx. Let me try substitution y = x -1. Then, x = y +1, dx = dy, limits from y=-1 to y=1. The integral becomes ∫_{-1}^1 (y +1) arcsin(0.5√{(y+1)(1 - y)}) dy. As before, the term (y +1) arcsin(0.5√(1 - y²)) dy. The y term is odd, so integrates to zero, leaving ∫_{-1}^1 arcsin(0.5√(1 - y²)) dy = 2 ∫₀¹ arcsin(0.5√(1 - y²)) dy. Then, substitution y = sinθ, leading to 2 ∫₀^{π/2} arcsin(0.5 cosθ) cosθ dθ. Then, integrating by parts, leading to the same result. So, the analytical result is √3 - π/3. Therefore, the exact answer is √3 - π/3, and the numerical approximation is approximately 0.6848532564. So, the final answer should be {"answer": "\sqrt{3} - \dfrac{\pi}{3}", "numerical_answer": 0.6848532564} but in the required JSON format.
</think>

{"answer": "\\sqrt{3} - \\dfrac{\\pi}{3}", "numerical_answer": 0.6848532564}