To evaluate

  I = ∫₀∞ 1/(eˣ + 1) dx,

we begin by making a substitution. Let u = e^(–x); then du/dx = –e^(–x) = –u, so that dx = –du/u. When x = 0, we have u = e⁰ = 1, and as x → ∞, u = e^(–∞) = 0. The integral becomes

  I = ∫ₓ₌₀∞ 1/(eˣ + 1) dx
    = ∫ᵤ₌₁⁰ 1/(1/u + 1) (–du/u).

Notice that 1/(1/u + 1) = 1/((1 + u)/u) = u/(1 + u). Therefore, the expression simplifies as follows:

  I = ∫₁⁰ (u/(1 + u)) (–du/u) = –∫₁⁰ 1/(1 + u) du.

Changing the limits from 1 to 0 (or equivalently reversing the limits) gives

  I = ∫₀¹ 1/(1 + u) du.

This integral can now be computed directly:

  I = ∫₀¹ 1/(1 + u) du = ln|1 + u| evaluated from u = 0 to u = 1
    = ln(2) − ln(1) = ln 2.

Thus, the exact answer is ln 2.

For a numerical approximation, note that ln 2 ≈ 0.6931471806 (to 10 decimal places).

{"answer": "\\ln 2", "numerical_answer": "0.6931471806"}