Let’s tackle the given integral:

\[
I = \int_{0}^{2} \frac{x^{-1/2}(2-x)^{-1/2}}{\sqrt{1 + x(2-x)}} T_3\left(\sqrt{1 + x(2-x)}\right) dx
\]

where \( T_3(y) \) is the 3rd Chebyshev polynomial of the first kind:
\[
T_3(y) = 4y^3 - 3y
\]

Let’s proceed step by step:

---

**Step 1: Substitute and simplify**

Let \( y = \sqrt{1 + x(2-x)} \).

First, compute \( 1 + x(2-x) \):

\[
1 + x(2-x) = 1 + 2x - x^2 = -(x^2 - 2x - 1)
\]

But what’s more useful is to parameterize the problem to simplify the limits and integrand.

Let’s try substituting \( x = 2\sin^2\theta \), with \( x \in [0,2] \Rightarrow \theta \in [0, \pi/2] \):

- \( dx = 4\sin\theta \cos\theta \, d\theta = 2\sin2\theta\, d\theta \)
- \( x^{-1/2} = (2\sin^2\theta)^{-1/2} = 2^{-1/2} \sin^{-1}\theta \)
- \( 2-x = 2-2\sin^2\theta = 2\cos^2\theta \implies (2-x)^{-1/2} = 2^{-1/2} \cos^{-1}\theta \)
- Therefore \( x^{-1/2}(2-x)^{-1/2} dx = 2^{-1} \sin^{-1}\theta \cos^{-1}\theta \cdot 2\sin2\theta d\theta = \sin2\theta \cdot \sin^{-1}\theta \cos^{-1}\theta d\theta \)

But \( \sin2\theta = 2\sin\theta \cos\theta \). So,

\[
x^{-1/2}(2-x)^{-1/2} dx = (2\sin\theta \cos\theta)\cdot \frac{d\theta}{\sin\theta \cos\theta} = 2 d\theta
\]

So the measure simplifies! Now,

\[
1 + x(2-x) = 1 + 2\sin^2\theta \cdot 2\cos^2\theta = 1 + 4\sin^2\theta\cos^2\theta = 1 + \sin^2 2\theta
\]

Therefore,

\[
y = \sqrt{1 + x(2-x)} = \sqrt{1 + \sin^2 2\theta}
\]

And finally, the integrand:

- Numerator: \( x^{-1/2}(2-x)^{-1/2} dx = 2 d\theta \)
- Denominator: \( \sqrt{1 + x(2-x)} = y \)
- Chebyshev: \( T_3(y) = 4y^3 -3y \)

So the total integrand becomes:

\[
I = \int_{x=0}^{2} \frac{x^{-1/2}(2-x)^{-1/2}}{y} T_3(y) dx = \int_{\theta=0}^{\pi/2} \frac{2}{y} T_3(y) d\theta
\]
\[
=2\int_0^{\pi/2} \frac{4y^3-3y}{y} d\theta = 2\int_0^{\pi/2} [4y^2-3] d\theta
\]

Next, recall that \( y^2 = 1 + \sin^2 2\theta \):

\[
I = 2\int_0^{\pi/2} [4(1+\sin^2 2\theta) - 3] d\theta
= 2\int_0^{\pi/2} [4 + 4\sin^2 2\theta - 3] d\theta
= 2\int_0^{\pi/2} [1 + 4\sin^2 2\theta] d\theta
\]

\[
I = 2\left( \int_0^{\pi/2} d\theta + 4\int_0^{\pi/2} \sin^2 2\theta d\theta \right )
= 2 \left( \frac{\pi}{2} + 4\int_0^{\pi/2} \sin^2 2\theta d\theta \right)
\]

Let’s now compute \( \int_0^{\pi/2} \sin^2 2\theta d\theta \):

Recall \( \sin^2 x = \frac{1-\cos 2x}{2} \), so

\[
\sin^2 2\theta = \frac{1 - \cos 4\theta}{2}
\]

So,

\[
\int_0^{\pi/2} \sin^2 2\theta d\theta = \int_0^{\pi/2} \frac{1 - \cos 4\theta}{2} d\theta = \frac{1}{2}\int_0^{\pi/2} d\theta - \frac{1}{2}\int_0^{\pi/2} \cos 4\theta d\theta
\]

Integrate:

- \( \int_0^{\pi/2} d\theta = \frac{\pi}{2} \)
- \( \int_0^{\pi/2} \cos 4\theta d\theta = \left.\frac{\sin 4\theta}{4}\right|_0^{\pi/2} = \frac{\sin 2\pi - \sin 0}{4} = 0 \)

So,

\[
\int_0^{\pi/2} \sin^2 2\theta d\theta = \frac{1}{2} \cdot \frac{\pi}{2} - \frac{1}{2} \cdot 0 = \frac{\pi}{4}
\]

Now substitute back:

\[
I = 2 \left(\frac{\pi}{2} + 4\cdot \frac{\pi}{4} \right) = 2\left(\frac{\pi}{2} + \pi\right) = 2 \cdot \frac{3\pi}{2} = 3\pi
\]

---

**Step 2: Numerical Approximation**

\[
I = 3\pi \approx 3 \times 3.1415926536 = 9.4247779608
\]

---

**Final Answer in JSON:**

```json
{"answer": "3\\pi", "numerical_answer": "9.4247779608"}
```