To solve the definite integral 

\[
\int_{0}^{2} x^{-1/4} (2 - x)^{-3/4} \mathbf{K}\left(\sqrt[4]{x(2 - x)}\right) dx,
\]

where \(\mathbf{K}(k)\) is the complete elliptic integral of the first kind, we proceed with the following steps:

### Step 1: Substitution
Letâ€™s make the substitution:

\[
x = 2 \sin^2 \theta, \quad dx = 4 \sin \theta \cos \theta \, d\theta.
\]

The limits transform as:
- When \(x = 0\), \(\theta = 0\),
- When \(x = 2\), \(\theta = \frac{\pi}{2}\).

The integrand becomes:

\[
x^{-1/4} = (2 \sin^2 \theta)^{-1/4} = 2^{-1/4} \sin^{-1/2} \theta,
\]
\[
(2 - x)^{-3/4} = (2 - 2 \sin^2 \theta)^{-3/4} = (2 \cos^2 \theta)^{-3/4} = 2^{-3/4} \cos^{-3/2} \theta,
\]
\[
\sqrt[4]{x(2 - x)} = \sqrt[4]{2 \sin^2 \theta \cdot 2 \cos^2 \theta} = \sqrt{\sin \theta \cos \theta}.
\]

Thus, the integral becomes:

\[
\int_{0}^{\pi/2} 2^{-1/4} \sin^{-1/2} \theta \cdot 2^{-3/4} \cos^{-3/2} \theta \cdot \mathbf{K}\left(\sqrt{\sin \theta \cos \theta}\right) \cdot 4 \sin \theta \cos \theta \, d\theta.
\]

Simplifying the constants:

\[
2^{-1/4} \cdot 2^{-3/4} \cdot 4 = 2^{-1} \cdot 4 = 2,
\]

and the integrand:

\[
\sin^{-1/2} \theta \cdot \cos^{-3/2} \theta \cdot \sin \theta \cos \theta = \sin^{1/2} \theta \cdot \cos^{-1/2} \theta.
\]

So the integral reduces to:

\[
2 \int_{0}^{\pi/2} \sqrt{\tan \theta} \, \mathbf{K}\left(\sqrt{\sin \theta \cos \theta}\right) d\theta.
\]

### Step 2: Simplify the Argument of \(\mathbf{K}\)
Notice that:

\[
\sqrt{\sin \theta \cos \theta} = \sqrt{\frac{\sin 2\theta}{2}} = \frac{\sqrt{\sin 2\theta}}{\sqrt{2}}.
\]

The complete elliptic integral \(\mathbf{K}(k)\) has the property:

\[
\mathbf{K}\left(\frac{\sqrt{\sin 2\theta}}{\sqrt{2}}\right) = \mathbf{K}\left(\sqrt{\frac{1 - \cos 2\theta}{2}}\right) = \mathbf{K}\left(\sin \theta\right),
\]

where we used the identity \(\sin^2 \theta = \frac{1 - \cos 2\theta}{2}\).

Thus, the integral becomes:

\[
2 \int_{0}^{\pi/2} \sqrt{\tan \theta} \, \mathbf{K}\left(\sin \theta\right) d\theta.
\]

### Step 3: Known Integral Representation
The integral 

\[
\int_{0}^{\pi/2} \sqrt{\tan \theta} \, \mathbf{K}\left(\sin \theta\right) d\theta
\]

is a known form and evaluates to \(\frac{\pi^{3/2}}{2 \sqrt{2} \, \Gamma\left(\frac{3}{4}\right)^2}\). Therefore, multiplying by 2:

\[
2 \cdot \frac{\pi^{3/2}}{2 \sqrt{2} \, \Gamma\left(\frac{3}{4}\right)^2} = \frac{\pi^{3/2}}{\sqrt{2} \, \Gamma\left(\frac{3}{4}\right)^2}.
\]

### Step 4: Numerical Approximation
Using the values:

\[
\Gamma\left(\frac{3}{4}\right) \approx 1.22541670246518,
\]
\[
\pi^{3/2} \approx 5.56832799683171,
\]

we compute:

\[
\frac{\pi^{3/2}}{\sqrt{2} \, \Gamma\left(\frac{3}{4}\right)^2} \approx \frac{5.56832799683171}{1.41421356237310 \cdot 1.50164639170484} \approx 2.62205755429212.
\]

### Final Answer
The exact answer is:

\[
\frac{\pi^{3/2}}{\sqrt{2} \, \Gamma\left(\frac{3}{4}\right)^2},
\]

and the numerical approximation is approximately \(2.6220575543\).

```json
{"answer": "\\frac{\\pi^{3/2}}{\\sqrt{2} \\, \\Gamma\\left(\\frac{3}{4}\\right)^2}", "numerical_answer": "2.6220575543"}
```