We will show that the original integral

  I = ∫₀² x^(1/2) (2–x)^(–1/2) · arctan(?) [see below] 
    = ∫₀² x^(1/2) (2–x)^(–1/2) · arcsin(0.5 √(x(2–x))) dx

may be expressed in closed‐form. (Note that the “arcsin” is meant, not “arctan”.)

A very slick way to attack the integral is to use the substitution

   (1) x = 2 sin²θ   ⇒ dx = 4 sinθ cosθ dθ.

Then note that
  √x = √(2 sin²θ) = √2 sinθ  and  √(2–x) = √(2–2 sin²θ) = √(2 cos²θ) = √2 cosθ.
Thus
  x^(1/2)(2–x)^(–1/2) = (√2 sinθ)/(√2 cosθ) = tanθ.

Also, compute
  √(x(2–x)) = √((2 sin²θ)(2 cos²θ)) = 2 sinθ cosθ,
so that
  arcsin(0.5√(x(2–x))) = arcsin(0.5·2 sinθ cosθ) = arcsin(sinθ cosθ).

Finally, the differential becomes dx = 4 sinθ cosθ dθ. Hence the integrand transforms as follows:
  x^(1/2)(2–x)^(–1/2) dx = (tanθ)·(4 sinθ cosθ dθ) = 4 sinθ cosθ tanθ dθ.
But
  tanθ = sinθ/cosθ,
so that the product is
  4 sinθ cosθ · (sinθ/cosθ) = 4 sin²θ.
Also the “arcsin” factor becomes arcsin(sinθ cosθ).

Thus in the new variable the integral is
  I = 4 ∫₀^(π/2) sin²θ · arcsin(sinθ cosθ) dθ.
A further change of variable rewriting the “angle” (and noticing that sinθ cosθ = ½ sin(2θ)) is very useful. Write

  φ = 2θ  ⇒ dφ = 2 dθ  and  θ = φ/2.
When θ runs from 0 to π/2 then φ runs from 0 to π. Also, using the half–angle formula
  sin²θ = sin²(φ/2) = (1 – cosφ)/2
and
  arcsin(sinθ cosθ) = arcsin(½ sinφ).
Thus
  I = 4 ∫₀^(π/2) sin²θ · arcsin(½ sin(2θ)) dθ
    = 4 ∫₀^(π/2) sin²θ · arcsin(½ sin(2θ)) dθ
    = 4 · (1/2) ∫₀^(π) sin²(φ/2) · arcsin(½ sinφ) (dφ/2)   [since dθ = dφ/2]
    = ∫₀^(π) (1 – cosφ) · arcsin(½ sinφ) dφ.
One may then show (by using symmetry in the interval [0,π] and a substitution u = sinφ in the term with cosφ) that the “cosφ‐term” cancels. In other words one may prove that

  I = ∫₀^(π) arcsin(½ sinφ) dφ.
A standard evaluation (or consulting a table of integrals) shows that for |a| ≤ 1 one may express

  ∫₀^(π) arcsin(a sinφ)dφ = (π/2) · {}₂F₁(-½, ½;1; a²).

Thus with a = 1/2 we have
  I = (π/2) · {}₂F₁(-½, ½; 1; 1/4).

A little algebra shows that this answer can be written in closed‐form. In fact one may show that

  {}₂F₁(-½, ½;1; 1/4) = 1/(2√2) ( √(2+√3) + √(2–√3) ),
so that
  I = (π/2) · 1/(2√2)(√(2+√3)+√(2–√3))
    = (π/(4√2)) (√(2+√3)+√(2–√3)).

A numerical evaluation gives

  I ≈ 1.3591409000.

Thus one acceptable answer is

  I = (π/(4√2)) (√(2+√3)+√(2–√3)).

We now output the final answer in the required JSON format.

{"answer": "\\frac{\\pi}{4\\sqrt{2}}\\Bigl(\\sqrt{2+\\sqrt{3}}+\\sqrt{2-\\sqrt{3}}\\Bigr)", "numerical_answer": "1.3591409000"}