

To solve the definite integral \(\int_{0}^{1} \frac{x^3 + x + 1}{3x^2 - 3x + 4} \, dx\), we follow these steps:

### Step 1: Polynomial Long Division
The integrand is a rational function where the numerator (degree 3) has a higher degree than the denominator (degree 2). We perform polynomial long division to simplify the integrand:

Dividing \(x^3 + x + 1\) by \(3x^2 - 3x + 4\):
- The first term of the quotient is \(\frac{1}{3}x\). Multiplying the denominator by \(\frac{1}{3}x\) gives \(x^3 - x^2 + \frac{4}{3}x\).
- Subtracting this from the numerator leaves a remainder of \(x^2 - \frac{1}{3}x + 1\).
- The next term of the quotient is \(\frac{1}{3}\). Multiplying the denominator by \(\frac{1}{3}\) gives \(x^2 - x + \frac{4}{3}\).
- Subtracting this from the remainder leaves a final remainder of \(\frac{2}{3}x - \frac{1}{3}\).

Thus, the integrand simplifies to:
\[
\frac{x^3 + x + 1}{3x^2 - 3x + 4} = \frac{1}{3}x + \frac{1}{3} + \frac{\frac{2}{3}x - \frac{1}{3}}{3x^2 - 3x + 4}
\]

### Step 2: Split the Integral
We split the integral into three parts:
\[
\int_{0}^{1} \left( \frac{1}{3}x + \frac{1}{3} + \frac{\frac{2}{3}x - \frac{1}{3}}{3x^2 - 3x + 4} \right) dx = \int_{0}^{1} \frac{1}{3}x \, dx + \int_{0}^{1} \frac{1}{3} \, dx + \int_{0}^{1} \frac{\frac{2}{3}x - \frac{1}{3}}{3x^2 - 3x + 4} \, dx
\]

### Step 3: Evaluate Each Integral
1. **First Integral**: \(\int_{0}^{1} \frac{1}{3}x \, dx\)
   \[
   \int \frac{1}{3}x \, dx = \frac{1}{6}x^2 \bigg|_{0}^{1} = \frac{1}{6}(1^2 - 0^2) = \frac{1}{6}
   \]

2. **Second Integral**: \(\int_{0}^{1} \frac{1}{3} \, dx\)
   \[
   \int \frac{1}{3} \, dx = \frac{1}{3}x \bigg|_{0}^{1} = \frac{1}{3}(1 - 0) = \frac{1}{3}
   \]

3. **Third Integral**: \(\int_{0}^{1} \frac{\frac{2}{3}x - \frac{1}{3}}{3x^2 - 3x + 4} \, dx\)
   Let \(u = 3x^2 - 3x + 4\), so \(du = (6x - 3)dx = 3(2x - 1)dx\). Thus, \((2x - 1)dx = \frac{du}{3}\). The integrand becomes:
   \[
   \frac{\frac{2}{3}x - \frac{1}{3}}{u} dx = \frac{1}{3} \cdot \frac{2x - 1}{u} dx = \frac{1}{3} \cdot \frac{du}{3u} = \frac{1}{9} \cdot \frac{du}{u}
   \]
   Integrating gives:
   \[
   \frac{1}{9} \ln|u| \bigg|_{0}^{1} = \frac{1}{9} \left( \ln(3(1)^2 - 3(1) + 4) - \ln(3(0)^2 - 3(0) + 4) \right) = \frac{1}{9} (\ln 4 - \ln 4) = 0
   \]

### Step 4: Combine Results
Adding the three integrals:
\[
\frac{1}{6} + \frac{1}{3} + 0 = \frac{1}{6} + \frac{2}{6} = \frac{3}{6} = \frac{1}{2}
\]

### Numerical Approximation
The exact result is \(\frac{1}{2}\), which is \(0.5\) when rounded to 10 decimal places.

{"answer": "\(\frac{1}{2}\)", "numerical_answer": "0.5000000000"}