
To solve the definite integral \(\int_0^1\left(\frac{x^2}{2-x^2}+\sqrt{\frac{2x}{x+1}}\right)\:dx\), we split it into two parts: \(I_1 = \int_0^1 \frac{x^2}{2-x^2}\,dx\) and \(I_2 = \int_0^1 \sqrt{\frac{2x}{x+1}}\,dx\).

### Step 1: Compute \(I_1\)
Rewrite the integrand using algebraic manipulation:
\[
\frac{x^2}{2-x^2} = -1 + \frac{2}{2-x^2}
\]
Integrate term by term:
\[
I_1 = \int_0^1 \left(-1 + \frac{2}{2-x^2}\right) dx = \int_0^1 -1\,dx + 2\int_0^1 \frac{1}{2-x^2}\,dx
\]
The first integral is straightforward:
\[
\int_0^1 -1\,dx = -1
\]
For the second integral, use the standard result \(\int \frac{1}{a^2 - x^2}\,dx = \frac{1}{2a}\ln\left|\frac{a+x}{a-x}\right| + C\) with \(a = \sqrt{2}\):
\[
2\int_0^1 \frac{1}{2-x^2}\,dx = 2 \cdot \frac{1}{2\sqrt{2}} \ln\left(\frac{\sqrt{2}+x}{\sqrt{2}-x}\right) \bigg|_0^1 = \frac{1}{\sqrt{2}} \ln\left(\frac{\sqrt{2}+1}{\sqrt{2}-1}\right)
\]
Simplify \(\frac{\sqrt{2}+1}{\sqrt{2}-1} = 3 + 2\sqrt{2}\) (by rationalizing the denominator). Thus:
\[
I_1 = -1 + \frac{1}{\sqrt{2}} \ln(3 + 2\sqrt{2})
\]

### Step 2: Compute \(I_2\)
Use the substitution \(t = \sqrt{\frac{x}{x+1}}\), so \(x = \frac{t^2}{1-t^2}\) and \(dx = \frac{2t}{(1-t^2)^2}dt\). The integrand transforms as:
\[
\sqrt{\frac{2x}{x+1}} = \sqrt{2}t
\]
The limits change from \(x=0\) ( \(t=0\) ) to \(x=1\) ( \(t=1/\sqrt{2}\) ). Thus:
\[
I_2 = \int_0^{1/\sqrt{2}} \sqrt{2}t \cdot \frac{2t}{(1-t^2)^2} dt = 2\sqrt{2} \int_0^{1/\sqrt{2}} \frac{t^2}{(1-t^2)^2} dt
\]
Integrate \(\frac{t^2}{(1-t^2)^2}\) using integration by parts or simplification, leading to:
\[
\int \frac{t^2}{(1-t^2)^2} dt = \frac{t}{2(1-t^2)} - \frac{1}{4}\ln\left(\frac{1+t}{1-t}\right) + C
\]
Evaluating from \(0\) to \(1/\sqrt{2}\) and simplifying, we find:
\[
I_2 = 2 - \frac{\sqrt{2}}{2} \ln(3 + 2\sqrt{2})
\]

### Step 3: Combine \(I_1\) and \(I_2\)
Adding \(I_1\) and \(I_2\):
\[
I_1 + I_2 = \left(-1 + \frac{1}{\sqrt{2}} \ln(3 + 2\sqrt{2})\right) + \left(2 - \frac{\sqrt{2}}{2} \ln(3 + 2\sqrt{2})\right)
\]
The logarithmic terms cancel (since \(\frac{1}{\sqrt{2}} = \frac{\sqrt{2}}{2}\)), leaving:
\[
I_1 + I_2 = 1
\]

### Numerical Approximation
The exact result is \(1\), so the numerical approximation is \(1.0000000000\).

{"answer": "1", "numerical_answer": "1.0000000000"}