To solve the definite integral \(\int_{\frac{1}{8}}^{\frac{1}{4}} \frac{\ln(2x) \ln(4x) \ln(8x)}{x} \, dx\), we will follow the steps outlined.

### Step 1: Simplify the integrand

First, let's simplify the integrand \(\frac{\ln(2x) \ln(4x) \ln(8x)}{x}\).

Using the properties of logarithms:
\[
\ln(2x) = \ln 2 + \ln x
\]
\[
\ln(4x) = \ln 4 + \ln x = 2\ln 2 + \ln x
\]
\[
\ln(8x) = \ln 8 + \ln x = 3\ln 2 + \ln x
\]

Substitute these into the integrand:
\[
\frac{\ln(2x) \ln(4x) \ln(8x)}{x} = \frac{(\ln 2 + \ln x)(2\ln 2 + \ln x)(3\ln 2 + \ln x)}{x}
\]

### Step 2: Expand the product

Expand the product \((\ln 2 + \ln x)(2\ln 2 + \ln x)(3\ln 2 + \ln x)\):

\[
(\ln 2 + \ln x)(2\ln 2 + \ln x) = 2\ln^2 2 + \ln 2 \ln x + 2\ln 2 \ln x + \ln^2 x = 2\ln^2 2 + 3\ln 2 \ln x + \ln^2 x
\]

Now multiply this result by \((3\ln 2 + \ln x)\):

\[
(2\ln^2 2 + 3\ln 2 \ln x + \ln^2 x)(3\ln 2 + \ln x)
\]

Expanding this product:

\[
= 2\ln^2 2 \cdot 3\ln 2 + 2\ln^2 2 \cdot \ln x + 3\ln 2 \ln x \cdot 3\ln 2 + 3\ln 2 \ln x \cdot \ln x + \ln^2 x \cdot 3\ln 2 + \ln^2 x \cdot \ln x
\]

\[
= 6\ln^3 2 + 2\ln^2 2 \ln x + 9\ln^2 2 \ln x + 3\ln 2 \ln^2 x + 3\ln 2 \ln^2 x + \ln^3 x
\]

Combine like terms:

\[
= 6\ln^3 2 + (2\ln^2 2 \ln x + 9\ln^2 2 \ln x) + (3\ln 2 \ln^2 x + 3\ln 2 \ln^2 x) + \ln^3 x
\]

\[
= 6\ln^3 2 + 11\ln^2 2 \ln x + 6\ln 2 \ln^2 x + \ln^3 x
\]

### Step 3: Integrate term by term

Now, integrate each term separately:

\[
\int_{\frac{1}{8}}^{\frac{1}{4}} \frac{6\ln^3 2}{x} \, dx = 6\ln^3 2 \int_{\frac{1}{8}}^{\frac{1}{4}} \frac{1}{x} \, dx = 6\ln^3 2 \left[ \ln x \right]_{\frac{1}{8}}^{\frac{1}{4}} = 6\ln^3 2 (\ln \frac{1}{4} - \ln \frac{1}{8})
\]

\[
= 6\ln^3 2 (\ln 2 - 2\ln 2) = 6\ln^3 2 (-\ln 2) = -6\ln^4 2
\]

\[
\int_{\frac{1}{8}}^{\frac{1}{4}} \frac{11\ln^2 2 \ln x}{x} \, dx = 11\ln^2 2 \int_{\frac{1}{8}}^{\frac{1}{4}} \frac{\ln x}{x} \, dx = 11\ln^2 2 \left[ \frac{(\ln x)^2}{2} \right]_{\frac{1}{8}}^{\frac{1}{4}}
\]

\[
= 11\ln^2 2 \left( \frac{(\ln \frac{1}{4})^2}{2} - \frac{(\ln \frac{1}{8})^2}{2} \right) = 11\ln^2 2 \left( \frac{(-2\ln 2)^2}{2} - \frac{(-3\ln 2)^2}{2} \right)
\]

\[
= 11\ln^2 2 \left( \frac{4\ln^2 2}{2} - \frac{9\ln^2 2}{2} \right) = 11\ln^2 2 \left( 2\ln^2 2 - \frac{9\ln^2 2}{2} \right) = 11\ln^2 2 \left( -\frac{5\ln^2 2}{2} \right) = -\frac{55\ln^4 2}{2}
\]

\[
\int_{\frac{1}{8}}^{\frac{1}{4}} \frac{6\ln 2 \ln^2 x}{x} \, dx = 6\ln 2 \int_{\frac{1}{8}}^{\frac{1}{4}} \frac{\ln^2 x}{x} \, dx = 6\ln 2 \left[ \frac{(\ln x)^3}{3} \right]_{\frac{1}{8}}^{\frac{1}{4}}
\]

\[
= 6\ln 2 \left( \frac{(\ln \frac{1}{4})^3}{3} - \frac{(\ln \frac{1}{8})^3}{3} \right) = 6\ln 2 \left( \frac{(-2\ln 2)^3}{3} - \frac{(-3\ln 2)^3}{3} \right)
\]

\[
= 6\ln 2 \left( \frac{-8\ln^3 2}{3} - \frac{-27\ln^3 2}{3} \right) = 6\ln 2 \left( \frac{19\ln^3 2}{3} \right) = 38\ln^4 2
\]

\[
\int_{\frac{1}{8}}^{\frac{1}{4}} \frac{\ln^3 x}{x} \, dx = \left[ \frac{(\ln x)^4}{4} \right]_{\frac{1}{8}}^{\frac{1}{4}} = \frac{(\ln \frac{1}{4})^4}{4} - \frac{(\ln \frac{1}{8})^4}{4}
\]

\[
= \frac{(-2\ln 2)^4}{4} - \frac{(-3\ln 2)^4}{4} = \frac{16\ln^4 2}{4} - \frac{81\ln^4 2}{4} = \frac{-65\ln^4 2}{4}
\]

### Step 4: Combine the results

Combine all the integrals:

\[
-6\ln^4 2 - \frac{55\ln^4 2}{2} + 38\ln^4 2 - \frac{65\ln^4 2}{4}
\]

Convert all terms to a common denominator (4):

\[
-24\ln^4 2 - 110\ln^4 2 + 152\ln^4 2 - 65\ln^4 2 = (-24 - 110 + 152 - 65)\ln^4 2 = -47\ln^4 2
\]

### Step 5: Numerical approximation

Using \(\ln 2 \approx 0.69314718056\):

\[
\ln^4 2 \approx (0.69314718056)^4 \approx 0.2302585092994046
\]

\[
-47 \ln^4 2 \approx -47 \times 0.2302585092994046 \approx -10.822149936071916
\]

### Final Answer

\[
\boxed{
\begin{aligned}
\text{"answer": "-47\ln^4 2",} \\
\text{"numerical_answer": "-10.8221499361"}
\end{aligned}
}
\]