To solve the definite integral \(\int_0^1 \sqrt[3]{x} \left\lfloor \frac{1}{\sqrt[3]{x}} \right\rfloor \, dx\), we need to carefully analyze the integrand and break it down into manageable parts.

### Step 1: Analyze the integrand

The integrand is \(\sqrt[3]{x} \left\lfloor \frac{1}{\sqrt[3]{x}} \right\rfloor\). Let \( t = \sqrt[3]{x} \). Then \( x = t^3 \) and \( dx = 3t^2 dt \). The integral becomes:
\[
\int_0^1 \sqrt[3]{x} \left\lfloor \frac{1}{\sqrt[3]{x}} \right\rfloor \, dx = \int_0^1 t \left\lfloor \frac{1}{t} \right\rfloor \cdot 3t^2 \, dt = 3 \int_0^1 t^3 \left\lfloor \frac{1}{t} \right\rfloor \, dt.
\]

### Step 2: Break the integral into parts

The floor function \(\left\lfloor \frac{1}{t} \right\rfloor\) changes value at points where \(\frac{1}{t}\) is an integer. Let \( n = \left\lfloor \frac{1}{t} \right\rfloor \). Then \( n \leq \frac{1}{t} < n+1 \), which implies \( \frac{1}{n+1} < t \leq \frac{1}{n} \).

We can split the integral into parts where \( t \) ranges from \(\frac{1}{n+1}\) to \(\frac{1}{n}\) for \( n = 1, 2, 3, \ldots \).

\[
3 \int_0^1 t^3 \left\lfloor \frac{1}{t} \right\rfloor \, dt = 3 \sum_{n=1}^{\infty} \int_{\frac{1}{n+1}}^{\frac{1}{n}} t^3 n \, dt.
\]

### Step 3: Evaluate each part of the sum

For each \( n \), we have:
\[
\int_{\frac{1}{n+1}}^{\frac{1}{n}} t^3 n \, dt = n \int_{\frac{1}{n+1}}^{\frac{1}{n}} t^3 \, dt.
\]

The integral of \( t^3 \) is:
\[
\int t^3 \, dt = \frac{t^4}{4}.
\]

Evaluating this from \(\frac{1}{n+1}\) to \(\frac{1}{n}\):
\[
n \left[ \frac{t^4}{4} \right]_{\frac{1}{n+1}}^{\frac{1}{n}} = n \left( \frac{\left(\frac{1}{n}\right)^4}{4} - \frac{\left(\frac{1}{n+1}\right)^4}{4} \right) = n \left( \frac{1}{4n^4} - \frac{1}{4(n+1)^4} \right).
\]

Simplifying:
\[
n \left( \frac{1}{4n^4} - \frac{1}{4(n+1)^4} \right) = \frac{n}{4n^4} - \frac{n}{4(n+1)^4} = \frac{1}{4n^3} - \frac{n}{4(n+1)^4}.
\]

### Step 4: Sum the series

The integral becomes:
\[
3 \sum_{n=1}^{\infty} \left( \frac{1}{4n^3} - \frac{n}{4(n+1)^4} \right).
\]

This can be split into two sums:
\[
3 \left( \frac{1}{4} \sum_{n=1}^{\infty} \frac{1}{n^3} - \frac{1}{4} \sum_{n=1}^{\infty} \frac{n}{(n+1)^4} \right).
\]

The first sum is a known series:
\[
\sum_{n=1}^{\infty} \frac{1}{n^3} = \zeta(3),
\]
where \(\zeta(3)\) is the Riemann zeta function evaluated at 3.

For the second sum, we can reindex \( m = n+1 \):
\[
\sum_{n=1}^{\infty} \frac{n}{(n+1)^4} = \sum_{m=2}^{\infty} \frac{m-1}{m^4} = \sum_{m=2}^{\infty} \left( \frac{1}{m^3} - \frac{1}{m^4} \right).
\]

This can be split into:
\[
\sum_{m=2}^{\infty} \frac{1}{m^3} - \sum_{m=2}^{\infty} \frac{1}{m^4} = \left( \zeta(3) - 1 \right) - \left( \zeta(4) - 1 \right).
\]

Combining these results:
\[
3 \left( \frac{1}{4} \zeta(3) - \frac{1}{4} \left( \zeta(3) - 1 - \zeta(4) + 1 \right) \right) = 3 \left( \frac{1}{4} \zeta(3) - \frac{1}{4} \left( \zeta(3) - \zeta(4) \right) \right).
\]

Simplifying:
\[
3 \left( \frac{1}{4} \zeta(3) - \frac{1}{4} \zeta(3) + \frac{1}{4} \zeta(4) \right) = 3 \left( \frac{1}{4} \zeta(4) \right) = \frac{3}{4} \zeta(4).
\]

Since \(\zeta(4) = \frac{\pi^4}{90}\):
\[
\frac{3}{4} \cdot \frac{\pi^4}{90} = \frac{3 \pi^4}{360} = \frac{\pi^4}{120}.
\]

### Step 5: Numerical approximation

Using \(\pi \approx 3.141592653589793\):
\[
\pi^4 \approx 97.40909103400244,
\]
\[
\frac{\pi^4}{120} \approx \frac{97.40909103400244}{120} \approx 0.8117424252833537.
\]

### Final Answer

\[
\boxed{
\begin{aligned}
\text{"answer": "}\frac{\pi^4}{120}\text{"}, \\
\text{"numerical_answer": "0.8117424253"}
\end{aligned}
}
\]