We wish to evaluate

  I = ∫₀¹ (1/x) · arccos(x) · [arcsin(x)]² dx.

Step 1. Change of Variable

A good substitution is to let

  u = arcsin x,  so that  x = sin u  and  dx = cos u du.

When x goes from 0 to 1, u goes from 0 to π/2. Also note that

  arcsin x = u   and
  arccos x = arccos(sin u).

For 0 ≤ u ≤ π/2 we have sin u = cos(π/2 – u), so that (with the output in the range [0, π/2]) 
  arccos(sin u) = π/2 – u.

Substitute into the integrand. Also note that 
  1/x = 1/sin u.
Thus the integral becomes

  I = ∫₀^(π/2) (1/sin u) · (π/2 – u) · u² · cos u du.

But cos u/sin u = cot u. Hence

  I = ∫₀^(π/2) u² (π/2 – u) cot u du.

It is best to split the product:
  I = (π/2) ∫₀^(π/2) u² cot u du – ∫₀^(π/2) u³ cot u du.
Define
  I₁ = ∫₀^(π/2) u² cot u du  and  I₂ = ∫₀^(π/2) u³ cot u du.
Then,
  I = (π/2) I₁ – I₂.

Step 2. Expressing Cotangent as a Derivative

Observe that
  d/du [ln(sin u)] = cot u.
Thus we can write each of I₁ and I₂ as an integral of the form

  I₁ = ∫₀^(π/2) u² d[ln(sin u)]
  I₂ = ∫₀^(π/2) u³ d[ln(sin u)].

We integrate by parts. In general, for any function f(u),
  ∫ f(u) d[ln(sin u)] = [f(u) ln(sin u)]₀^(π/2) – ∫₀^(π/2) f′(u) ln(sin u) du.
Since ln(sin u) vanishes at u = π/2 (because sin(π/2) = 1) and the boundary term vanishes at u = 0 (one may check that uᵏ ln(sin u) → 0 as u → 0), we obtain

  I₁ = – ∫₀^(π/2) (d/du (u²)) ln(sin u) du = –2 ∫₀^(π/2) u ln(sin u) du,
  I₂ = – ∫₀^(π/2) (d/du (u³)) ln(sin u) du = –3 ∫₀^(π/2) u² ln(sin u) du.

Define
  J₁ = ∫₀^(π/2) u ln(sin u) du  and  J₂ = ∫₀^(π/2) u² ln(sin u) du.
Then
  I₁ = –2J₁   and  I₂ = –3J₂.

Thus our original I becomes

  I = (π/2)(–2J₁) – (–3J₂) = –π J₁ + 3J₂.

Step 3. Evaluate J₁ and J₂ Using a Fourier Series Expansion

A well‐known expansion for 0 < u < π is

  ln(sin u) = – ln 2 – Σₘ₌₁^∞ (cos(2m u)/m).

We now use this expansion to write

  J₁ = ∫₀^(π/2) u ln(sin u) du 
     = – ln 2 ∫₀^(π/2) u du – Σₘ₌₁^∞ (1/m) ∫₀^(π/2) u cos(2m u) du.
Similarly,
  J₂ = ∫₀^(π/2) u² ln(sin u) du 
     = – ln 2 ∫₀^(π/2) u² du – Σₘ₌₁^∞ (1/m) ∫₀^(π/2) u² cos(2m u) du.

We compute the elementary integrals:
• ∫₀^(π/2) u du = (π/2)²/2 = π²/8.
• ∫₀^(π/2) u² du = (π/2)³/3 = π³/24.

Now, for the cosine integrals we proceed one by one.

A. Compute Aₘ = ∫₀^(π/2) u cos(2m u) du.
Integration by parts:
  Let v = u  ⇒ dv = du,
   dw = cos(2m u) du  ⇒ w = sin(2m u)/(2m).
Thus,
  Aₘ = [u sin(2m u)/(2m)]₀^(π/2) – ∫₀^(π/2) (sin(2m u)/(2m)) du.
At u = π/2, sin(π m) = 0 so the boundary is 0. Also,
  ∫₀^(π/2) sin(2m u) du = (1 – cos(mπ))/(2m).
Therefore,
  Aₘ = – [1/(2m)] · [(1 – cos(mπ))/(2m)] = – (1 – cos(mπ))/(4m²).
But cos(mπ) = (–1)ᵐ. Hence,
  Aₘ = – (1 – (–1)ᵐ)/(4m²).

B. Compute Bₘ = ∫₀^(π/2) u² cos(2m u) du.
Again, integrate by parts:
  Let v = u² (dv = 2u du) and dw = cos(2m u) du (w = sin(2m u)/(2m)).
Then,
  Bₘ = [u² sin(2m u)/(2m)]₀^(π/2) – ∫₀^(π/2) [2u sin(2m u)/(2m)] du 
    = [ (π/2)² sin(mπ)/(2m) ] – (1/m) ∫₀^(π/2) u sin(2m u) du.
Since sin(mπ) = 0, only the second term remains.
Now, denote Cₘ = ∫₀^(π/2) u sin(2m u) du.
Again by parts:
  Let r = u (dr = du) and dS = sin(2m u) du  (S = –cos(2m u)/(2m)).
Thus,
  Cₘ = [–u cos(2m u)/(2m)]₀^(π/2) + ∫₀^(π/2) cos(2m u)/(2m) du.
At u = π/2, this is –( (π/2) cos(mπ)/(2m).
The remaining integral:
  ∫₀^(π/2) cos(2m u) du = sin(2m u)/(2m)│₀^(π/2) = sin(mπ)/(2m)= 0.
Thus, Cₘ = – (π cos(mπ))/(4m).
Returning, we have
  Bₘ = – (1/m) Cₘ = π cos(mπ)/(4m²) = π (–1)ᵐ/(4m²).

Now plug these into the series for J₁ and J₂.

For J₁:
  J₁ = – ln2 · (π²/8) – Σₘ₌₁^∞ (1/m) Aₘ
    = – (π² ln2)/8 – Σₘ₌₁^∞ (1/m)[ – (1 – (–1)ᵐ)/(4m²)] 
    = – (π² ln2)/8 + (1/4) Σₘ₌₁^∞ (1 – (–1)ᵐ)/m³.
But
  Σₘ₌₁^∞ (1 – (–1)ᵐ)/m³ = Σₘ₌₁^∞ 1/m³ – Σₘ₌₁^∞ (–1)ᵐ/m³ = ζ(3) – (–(3/4)ζ(3))
    = ζ(3) + (3/4)ζ(3) = (7 ζ(3))/4,
using the standard result
  Σₘ₌₁^∞ (–1)^(m–1)/m³ = (3/4)ζ(3).
Thus,
  J₁ = – (π² ln2)/8 + (7 ζ(3))/(16).

For J₂:
  J₂ = – ln2 · (π³/24) – Σₘ₌₁^∞ (1/m) Bₘ
    = – (π³ ln2)/24 – Σₘ₌₁^∞ (1/m)[ π (–1)ᵐ/(4m²)]
    = – (π³ ln2)/24 – (π/4) Σₘ₌₁^∞ (–1)ᵐ/m³.
But
  Σₘ₌₁^∞ (–1)ᵐ/m³ = – Σₘ₌₁^∞ (–1)^(m–1)/m³ = – (3/4)ζ(3).
Thus,
  J₂ = – (π³ ln2)/24 + (3π ζ(3))/(16).

Step 4. Combine to Get I

Recall that we had

  I = – π J₁ + 3J₂.
Substitute the found expressions:
  I = – π [ – (π² ln2)/8 + (7 ζ(3))/(16) ] + 3 [ – (π³ ln2)/24 + (3π ζ(3))/(16) ]
    = π² ln2/8 – (7π ζ(3))/(16) – (3π³ ln2)/24 + (9π ζ(3))/(16).

Group the ln2–terms and the ζ(3)–terms:
• ln2–terms:
  π² ln2/8 – (3π³ ln2)/24.
Note that (3π³ ln2)/24 = π³ ln2/8. However, note π² and π³: actually, check the factors—
  π² ln2/8 and (3π³ ln2)/24 = π³ ln2/8. Since these have different powers of π they do not cancel unless π = 1. In fact, we must be careful: our ln2–terms involve π² vs. π³. Let us re‐examine the expressions:
  J₁ had a factor (π² ln2)/8 and J₂ had (π³ ln2)/24.
So then
  –π J₁ gives + (π³ ln2)/8,
  3 J₂ gives – (3π³ ln2)/24 = – (π³ ln2)/8.
Thus the ln2–terms cancel exactly.
• ζ(3)–terms:
  From –πJ₁ we have –π·(7 ζ(3))/(16) = – (7π ζ(3))/(16)
  From 3J₂ we have 3·(3π ζ(3))/(16) = (9π ζ(3))/(16)
Thus the total ζ(3) term is (–7π ζ(3)+9π ζ(3))/(16) = (2π ζ(3))/(16) = (π ζ(3))/8.

Thus the final answer is

  I = (π ζ(3))/8.

Step 5. Numerical Evaluation

Using the common approximations:
  π ≈ 3.1415926536  and  ζ(3) ≈ 1.2020569032,
we have
  I ≈ (3.1415926536 × 1.2020569032)/8.
First, compute the product:
  3.1415926536 × 1.2020569032 ≈ 3.77637325.
Then divide by 8:
  I ≈ 3.77637325/8 ≈ 0.4720466563.

Final Answer in JSON Format:

{"answer": "\\frac{\\pi \\zeta(3)}{8}", "numerical_answer": "0.4720466563"}