Let's tackle the definite integral:
\[
I = \int_0^1 \lfloor \log_{2023} x \rfloor dx
\]

### Step 1: Understanding the Floor

For \(0 < x < 1\), \(\log_{2023} x < 0\). The function \(\lfloor \log_{2023} x \rfloor\) is piecewise constant on intervals of the form
\[
2023^{-k-1} < x \leq 2023^{-k}
\]
for \(k = 0, 1, 2, \ldots\), with \(\lfloor\log_{2023} x\rfloor = -k-1\).

### Step 2: Determine the Range

For \(x=0\), \(\log_{2023}0 = -\infty\), while for \(x=1\), \(\log_{2023}1 = 0\). The function is only defined for \(x>0\), but the interval includes 0 as a limit.

Over \(x \in (2023^{-k-1}, 2023^{-k}]\), \(\lfloor \log_{2023} x \rfloor = -k-1\).

We seek all \(k\) such that \(2023^{-k} \geq 0\) and \(2023^{-k-1} < 1\). Since \(2023^{-k-1} \to 0\) as \(k \to \infty\), the sum is over all \(k \geq 0\).

### Step 3: Express as a Sum

The integral becomes:
\[
I = \sum_{k=0}^{\infty} \int_{2023^{-k-1}}^{2023^{-k}} (-k-1) dx
\]

### Step 4: Evaluate Each Piece

Each term:
\[
\int_{2023^{-k-1}}^{2023^{-k}} (-k-1) dx = (-k-1)\left[2023^{-k} - 2023^{-k-1}\right]
\]

### Step 5: Sum the Series

So,
\[
I = \sum_{k=0}^{\infty} (-k-1) (2023^{-k} - 2023^{-k-1})
\]

Let’s simplify \((2023^{-k} - 2023^{-k-1})\):
\[
2023^{-k-1} = \frac{1}{2023} \cdot 2023^{-k}
\implies 2023^{-k} - 2023^{-k-1} = \left(1 - \frac{1}{2023}\right) 2023^{-k} = \frac{2022}{2023} 2023^{-k}
\]

So,
\[
I = \sum_{k=0}^{\infty} (-k-1) \frac{2022}{2023} 2023^{-k}
\]
\[
= \frac{2022}{2023} \sum_{k=0}^{\infty} (-k-1) 2023^{-k}
\]

Let’s split \(-k-1 = -k - 1\):

\[
I = \frac{2022}{2023} \left(-\sum_{k=0}^{\infty} k\,2023^{-k} - \sum_{k=0}^{\infty} 2023^{-k}\right)
\]

Let’s compute the geometric series first:

- For \(S_1 = \sum_{k=0}^{\infty} 2023^{-k} = \frac{1}{1 - 1/2023} = \frac{2023}{2022}\)
  
- For \(S_2 = \sum_{k=0}^{\infty} k 2023^{-k}\):

Recall the formula:
\[\sum_{k=0}^{\infty} k r^k = \frac{r}{(1-r)^2},\]
for \(|r|<1\). Replace \(r = \frac{1}{2023}\):

\[
S_2 = \sum_{k=0}^{\infty} k \left(\frac{1}{2023}\right)^k = \frac{\frac{1}{2023}}{(1 - \frac{1}{2023})^2} = \frac{1/2023}{(2022/2023)^2} = \frac{1}{2023} \cdot \frac{2023^2}{2022^2} = \frac{2023}{2022^2}
\]

Plug these back in:

\[
I = \frac{2022}{2023} \left(- \frac{2023}{2022^2} - \frac{2023}{2022}\right)
\]
\[
= \frac{2022}{2023} \cdot \left(- \frac{2023 + 2023 \cdot 2022}{2022^2}\right)
\]
But let's combine:

- \(\frac{2023}{2022^2} + \frac{2023}{2022} = \frac{2023 + 2023 \cdot 2022}{2022^2} = \frac{2023(1 + 2022)}{2022^2} = \frac{2023 \cdot 2023}{2022^2}\)

So,

\[
I = -\frac{2022}{2023} \cdot \frac{2023 \cdot 2023}{2022^2} = -\frac{2022}{2023} \cdot \frac{2023^2}{2022^2} = -\frac{2023^2}{2022 \cdot 2023} = -\frac{2023}{2022}
\]

### Step 6: Final Expressions

**Exact value**:
\[
I = -\frac{2023}{2022}
\]

**Numerical approximation**:

\[
-\frac{2023}{2022} \approx -1.000494559
\]

---

```json
{"answer": "-\\frac{2023}{2022}", "numerical_answer": "-1.0004945590"}
```