<think>
Okay, let's see. I need to compute the definite integral from 64 to 729 of (x^(1/2))/(x^(1/2) - x^(1/3)) dx. Hmm, that looks a bit complicated with the different exponents. Maybe I can simplify the integrand first. 

The integrand is x^(1/2) divided by (x^(1/2) - x^(1/3)). Let me write that as [x^(1/2)] / [x^(1/2) - x^(1/3)]. To simplify this expression, perhaps I can factor out a common term from the denominator. Let's see, x^(1/3) is a common factor in the denominator. So, factoring x^(1/3) out of the denominator gives:

x^(1/3)(x^(1/2 - 1/3) - 1) = x^(1/3)(x^(1/6) - 1). Wait, let me check the exponent subtraction. 1/2 minus 1/3 is (3/6 - 2/6) = 1/6. So yes, the denominator becomes x^(1/3)(x^(1/6) - 1). 

So the integrand becomes [x^(1/2)] / [x^(1/3)(x^(1/6) - 1)] = x^(1/2 - 1/3) / (x^(1/6) - 1). Simplifying the exponent in the numerator: 1/2 - 1/3 = 1/6. So now it's x^(1/6)/(x^(1/6) - 1). 

Hmm, that's better. So the integral simplifies to the integral of x^(1/6)/(x^(1/6) - 1) dx from 64 to 729. Maybe substitution would work here. Let me set u = x^(1/6) - 1. Then du/dx would be (1/6)x^(-5/6). Let's compute that:

du/dx = (1/6)x^(-5/6) => du = (1/6)x^(-5/6) dx. Hmm, but in the integrand, I have x^(1/6) in the numerator. Let me see if I can express x^(1/6) in terms of u. Since u = x^(1/6) - 1, then x^(1/6) = u + 1. 

So, substituting, the integrand becomes (u + 1)/u. Then, the integral becomes ∫ (u + 1)/u * [something with du]. Wait, but I need to express dx in terms of du. Let's solve for dx. From du = (1/6)x^(-5/6) dx, so dx = 6x^(5/6) du. But x^(5/6) is (x^(1/6))^5. Since x^(1/6) = u + 1, then x^(5/6) = (u + 1)^5. Therefore, dx = 6(u + 1)^5 du. 

Putting it all together, the integral becomes ∫ [(u + 1)/u] * 6(u + 1)^5 du. Let's simplify that. The integrand is 6(u + 1)^6 / u du. So, expanding (u + 1)^6 might be tedious, but maybe there's a smarter way. Alternatively, perhaps we can perform polynomial division on (u + 1)^6 divided by u. Wait, (u + 1)^6 divided by u is the same as (u + 1)^6 * (1/u). Alternatively, expand (u + 1)^6 and then divide each term by u. 

But expanding (u + 1)^6 would take time. Let me recall the binomial theorem: (u + 1)^6 = Σ_{k=0}^6 C(6, k) u^k. So dividing by u gives Σ_{k=0}^6 C(6, k) u^{k - 1} = Σ_{k=0}^6 C(6, k) u^{k - 1}. Which is the same as u^{-1} + 6u^0 + 15u^1 + 20u^2 + 15u^3 + 6u^4 + u^5. 

Therefore, integrating term by term would be possible. But maybe there's a better substitution. Alternatively, perhaps we can split the fraction (u + 1)^6 / u into (u + 1)^6 / u. Let me note that (u + 1)^6 = u(u + 1)^5 + (u + 1)^5. Wait, maybe that's not helpful. Alternatively, perhaps we can write (u + 1)^6 / u as (u + 1)^6 / u = (u + 1)^5 * (u + 1)/u = (u + 1)^5 (1 + 1/u). Hmm, but that might not help. 

Alternatively, perhaps integrating (u + 1)^6 / u du. Let me consider expanding (u + 1)^6. Let's compute that:

(u + 1)^6 = u^6 + 6u^5 + 15u^4 + 20u^3 + 15u^2 + 6u + 1. Then, (u + 1)^6 / u = u^5 + 6u^4 + 15u^3 + 20u^2 + 15u + 6 + 1/u. 

So, the integral becomes 6 times the integral of [u^5 + 6u^4 + 15u^3 + 20u^2 + 15u + 6 + 1/u] du. That's manageable. Let's integrate term by term:

Integral of u^5 du = u^6 /6

Integral of 6u^4 du = 6*(u^5)/5 = (6/5)u^5

Integral of 15u^3 du = 15*(u^4)/4 = (15/4)u^4

Integral of 20u^2 du = 20*(u^3)/3 = (20/3)u^3

Integral of 15u du = 15*(u^2)/2 = (15/2)u^2

Integral of 6 du = 6u

Integral of 1/u du = ln|u|

So putting it all together, the integral is 6*[ (u^6)/6 + (6/5)u^5 + (15/4)u^4 + (20/3)u^3 + (15/2)u^2 + 6u + ln|u| ) ] + C. 

Simplify the coefficients:

The first term is 6*(u^6/6) = u^6

Then 6*(6/5)u^5 = (36/5)u^5

6*(15/4)u^4 = (90/4)u^4 = (45/2)u^4

6*(20/3)u^3 = (120/3)u^3 = 40u^3

6*(15/2)u^2 = (90/2)u^2 = 45u^2

6*6u = 36u

6*ln|u| = 6 ln|u|

So the antiderivative is:

u^6 + (36/5)u^5 + (45/2)u^4 + 40u^3 + 45u^2 + 36u + 6 ln|u| + C

Now, recall that u = x^(1/6) - 1. So we need to substitute back. Therefore, the antiderivative in terms of x is:

(x^(1/6) -1)^6 + (36/5)(x^(1/6) -1)^5 + (45/2)(x^(1/6) -1)^4 + 40(x^(1/6) -1)^3 + 45(x^(1/6) -1)^2 + 36(x^(1/6) -1) + 6 ln|x^(1/6) -1| + C

But this seems very complicated. Maybe there's a mistake here. Let me check the substitution steps again. Wait, perhaps expanding (u + 1)^6 and integrating term by term is correct, but maybe there's a smarter substitution. Let me think.

Alternatively, perhaps instead of substituting u = x^(1/6) -1, maybe a substitution t = x^(1/6). Let's try that. Let t = x^(1/6). Then x = t^6, so dx = 6t^5 dt. Then, the integrand is (x^(1/2))/(x^(1/2) - x^(1/3)) = (t^3)/(t^3 - t^2) = t^3/(t^2(t - 1)) = t/(t - 1). So the integrand simplifies to t/(t - 1). Therefore, the integral becomes ∫ [t/(t - 1)] * 6t^5 dt from t = x=64 to x=729. Let's compute the limits. When x=64, t=64^(1/6). 64 is 2^6, so t=2. When x=729, 729 is 3^6, so t=3. Therefore, the integral becomes 6 ∫ from t=2 to t=3 of [t/(t - 1)] * t^5 dt. Simplify the integrand: t/(t - 1) * t^5 = t^6/(t - 1). So the integral is 6 ∫_{2}^{3} t^6/(t - 1) dt. 

Hmm, integrating t^6/(t - 1). Maybe perform polynomial division here. Let's divide t^6 by t - 1. 

Using polynomial long division: t^6 divided by t - 1. 

First term: t^6 ÷ t = t^5. Multiply (t - 1) by t^5: t^6 - t^5. Subtract from t^6: 0 + t^5. Bring down the next terms (but there are none, so it's t^5). 

Next term: t^5 ÷ t = t^4. Multiply (t - 1) by t^4: t^5 - t^4. Subtract: t^5 - (t^5 - t^4) = t^4. 

Continue this process:

t^4 ÷ t = t^3. Multiply (t -1) by t^3: t^4 - t^3. Subtract: t^4 - (t^4 - t^3) = t^3.

t^3 ÷ t = t^2. Multiply (t -1) by t^2: t^3 - t^2. Subtract: t^3 - (t^3 - t^2) = t^2.

t^2 ÷ t = t. Multiply (t -1) by t: t^2 - t. Subtract: t^2 - (t^2 - t) = t.

t ÷ t = 1. Multiply (t -1) by 1: t -1. Subtract: t - (t -1) = 1.

So the division gives t^6/(t -1) = t^5 + t^4 + t^3 + t^2 + t +1 + 1/(t -1). 

Therefore, the integral becomes 6 ∫_{2}^{3} [t^5 + t^4 + t^3 + t^2 + t +1 + 1/(t -1)] dt. 

Now, integrating term by term:

Integral of t^5 dt = t^6/6

Integral of t^4 dt = t^5/5

Integral of t^3 dt = t^4/4

Integral of t^2 dt = t^3/3

Integral of t dt = t^2/2

Integral of 1 dt = t

Integral of 1/(t -1) dt = ln|t -1|

So putting it all together, the antiderivative is:

6*[ t^6/6 + t^5/5 + t^4/4 + t^3/3 + t^2/2 + t + ln|t -1| ] evaluated from t=2 to t=3.

Simplify the coefficients:

6*(t^6/6) = t^6

6*(t^5/5) = (6/5)t^5

6*(t^4/4) = (3/2)t^4

6*(t^3/3) = 2t^3

6*(t^2/2) = 3t^2

6*t = 6t

6*ln|t -1| = 6 ln|t -1|

So the antiderivative is:

t^6 + (6/5)t^5 + (3/2)t^4 + 2t^3 + 3t^2 + 6t + 6 ln|t -1| evaluated from 2 to 3.

Now compute F(3) - F(2):

First, compute F(3):

3^6 + (6/5)*3^5 + (3/2)*3^4 + 2*3^3 + 3*3^2 + 6*3 + 6 ln(3 -1)

Compute each term:

3^6 = 729

(6/5)*3^5 = (6/5)*243 = (1458)/5 = 291.6

(3/2)*3^4 = (3/2)*81 = 121.5

2*3^3 = 2*27 = 54

3*3^2 = 3*9 = 27

6*3 = 18

6 ln(2) ≈ 6*0.69314718056 ≈ 4.15888308336

Adding all together:

729 + 291.6 = 1020.6

1020.6 + 121.5 = 1142.1

1142.1 + 54 = 1196.1

1196.1 + 27 = 1223.1

1223.1 + 18 = 1241.1

1241.1 + 4.15888308336 ≈ 1245.25888308336

Now compute F(2):

2^6 + (6/5)*2^5 + (3/2)*2^4 + 2*2^3 + 3*2^2 + 6*2 + 6 ln(2 -1)

Compute each term:

2^6 = 64

(6/5)*2^5 = (6/5)*32 = 192/5 = 38.4

(3/2)*2^4 = (3/2)*16 = 24

2*2^3 = 2*8 = 16

3*2^2 = 3*4 = 12

6*2 = 12

6 ln(1) = 6*0 = 0

Adding all together:

64 + 38.4 = 102.4

102.4 + 24 = 126.4

126.4 + 16? Wait, 64 + 38.4 is 102.4, then +24 is 126.4, then +16 is 126.4 +16=142.4, then +12=154.4, then +12=166.4, then +0=166.4. Wait, let me check again:

Wait, 2^6 =64

(6/5)*2^5: 2^5=32, 6/5*32=192/5=38.4

(3/2)*2^4: 2^4=16, 3/2*16=24

2*2^3=2*8=16

3*2^2=3*4=12

6*2=12

6 ln(1)=0

So adding:

64 + 38.4 = 102.4

102.4 +24=126.4

126.4 +16=142.4

142.4 +12=154.4

154.4 +12=166.4

166.4 +0=166.4

So F(2) =166.4

Therefore, the definite integral is F(3) - F(2) ≈ 1245.25888308336 - 166.4 = 1245.25888308336 - 166.4 = 1078.85888308336. Wait, wait, wait. Wait, 1245.25888308336 minus 166.4 is 1078.85888308336. But let me check the numbers again.

Wait, F(3) was approximately 1245.25888308336 and F(2) is 166.4. So subtracting gives 1245.25888308336 - 166.4 = 1078.85888308336. But wait, this is the numerical approximation, but we need the exact value first. Let's compute the exact value.

First, compute F(3) exactly:

3^6 = 729

(6/5)*3^5 = 6/5 * 243 = 1458/5

(3/2)*3^4 = 3/2 *81 = 243/2

2*3^3 = 2*27=54

3*3^2=3*9=27

6*3=18

6 ln(2)

So F(3) = 729 + 1458/5 + 243/2 +54 +27 +18 +6 ln(2)

Convert all terms to fractions with denominator 10:

729 = 7290/10

1458/5 = 2916/10

243/2 = 1215/10

54 = 540/10

27 = 270/10

18 = 180/10

So adding:

7290/10 + 2916/10 = 10206/10

10206/10 + 1215/10 = 11421/10

11421/10 +540/10 = 11961/10

11961/10 +270/10 = 12231/10? Wait, 11961 +540=12501? Wait, no:

Wait, 7290 +2916=10206

10206 +1215=11421

11421 +540=11961

11961 +270=12231

12231 +180=12411

So total is 12411/10 +6 ln(2) = 1241.1 +6 ln(2)

Similarly, F(2) is:

2^6=64

(6/5)*2^5=6/5*32=192/5

(3/2)*2^4=3/2*16=24

2*2^3=16

3*2^2=12

6*2=12

6 ln(1)=0

So F(2)=64 +192/5 +24 +16 +12 +12 +0

Convert to fractions:

64 = 320/5

192/5 remains

24 = 120/5

16 = 80/5

12 = 60/5? Wait, 12=60/5? No, 12=60/5=12. Wait, 12=12*5/5=60/5. Similarly:

64 = 320/5

192/5

24 = 120/5

16 = 80/5

12 = 60/5

12 = 60/5

Adding all:

320/5 +192/5 =512/5

512/5 +120/5=632/5

632/5 +80/5=712/5

712/5 +60/5=772/5

772/5 +60/5=832/5

So F(2)=832/5 =166.4

Therefore, the exact value of the integral is [1241.1 +6 ln(2)] - 166.4 = 1241.1 -166.4 +6 ln(2) = 1074.7 +6 ln(2)

But 1241.1 -166.4 is 1074.7. So 1074.7 +6 ln(2). But 1074.7 is a decimal, but we need to express it as fractions. Let's see:

1241.1 is 12411/10, and 166.4 is 832/5. So 12411/10 -832/5 = 12411/10 -1664/10 = (12411 -1664)/10 = 10747/10. So the exact value is 10747/10 +6 ln(2). 

Therefore, the exact answer is 10747/10 +6 ln(2). But let's check if 10747/10 is correct. Wait, 12411 -1664=12411-1600=10811, then -64=10747. Yes. So 10747/10 is 1074.7. So the exact answer is 10747/10 +6 ln(2). 

Alternatively, we can write this as (10747/10) +6 ln(2). But perhaps simplify 10747/10. 10747 divided by 10 is 1074.7. So the exact answer is 1074.7 +6 ln(2). But to write this as an exact expression, we can keep it as 10747/10 +6 ln(2). Alternatively, combine the terms. But maybe it's better to leave it as fractions plus log terms. 

Alternatively, let's check the substitution steps again. Wait, when we did the substitution t =x^(1/6), then the integral became 6 ∫_{2}^{3} [t^6/(t -1)] dt, which after division became 6 ∫ [t^5 + t^4 + t^3 + t^2 + t +1 +1/(t -1)] dt. Then integrating term by term gives the antiderivative as t^6 + (6/5)t^5 + (3/2)t^4 +2t^3 +3t^2 +6t +6 ln|t -1| evaluated from 2 to 3. 

So the exact answer is [3^6 + (6/5)3^5 + (3/2)3^4 +2*3^3 +3*3^2 +6*3 +6 ln(2)] - [2^6 + (6/5)2^5 + (3/2)2^4 +2*2^3 +3*2^2 +6*2 +6 ln(1)]

Which simplifies to:

[729 + (6/5)(243) + (3/2)(81) +2*27 +3*9 +18 +6 ln2] - [64 + (6/5)(32) + (3/2)(16) +2*8 +3*4 +12 +0]

Calculating each term:

For t=3:

729 + (6/5)(243) =729 + 1458/5=729 +291.6=1020.6

(3/2)(81)=121.5

2*27=54

3*9=27

18

6 ln2

Summing these: 1020.6 +121.5=1142.1 +54=1196.1 +27=1223.1 +18=1241.1 +6 ln2

For t=2:

64 + (6/5)(32)=64 +192/5=64+38.4=102.4

(3/2)(16)=24

2*8=16

3*4=12

12

Summing:102.4 +24=126.4 +16=142.4 +12=154.4 +12=166.4

So the exact difference is (1241.1 +6 ln2) -166.4=1074.7 +6 ln2

But 1074.7 is 10747/10. So the exact answer is 10747/10 +6 ln2. 

Alternatively, we can write this as (10747 +60 ln2)/10, but perhaps it's better to leave it as 10747/10 +6 ln2. 

Now, to compute the numerical approximation. Let's compute 10747/10 which is 1074.7, and 6 ln2 ≈6*0.69314718056≈4.15888308336. So total is 1074.7 +4.15888308336≈1078.85888308336. Rounded to 10 decimal places, that's 1078.8588830834. 

But let me verify the exact answer again. Wait, when we did the substitution, the integral became 6 times the integral from t=2 to t=3 of t^6/(t-1) dt. Then after division, we integrated and got the antiderivative as t^6 + (6/5)t^5 + (3/2)t^4 +2t^3 +3t^2 +6t +6 ln|t-1|. Evaluated from 2 to 3. 

So the exact answer is:

[3^6 + (6/5)3^5 + (3/2)3^4 +2*3^3 +3*3^2 +6*3 +6 ln2] - [2^6 + (6/5)2^5 + (3/2)2^4 +2*2^3 +3*2^2 +6*2 +6 ln1]

Which is:

[729 + 1458/5 + 243/2 +54 +27 +18 +6 ln2] - [64 + 192/5 +24 +16 +12 +12 +0]

Converting all to fractions:

For t=3:

729 = 729/1

1458/5

243/2

54=54/1

27=27/1

18=18/1

6 ln2

Sum:

729 +1458/5 = (729*5 +1458)/5 = (3645 +1458)/5=5103/5

5103/5 +243/2= (5103*2 +243*5)/10= (10206 +1215)/10=11421/10=1142.1

1142.1 +54=1196.1

1196.1 +27=1223.1

1223.1 +18=1241.1

So total for t=3:1241.1 +6 ln2

For t=2:

64=64/1

192/5

24=24/1

16=16/1

12=12/1

12=12/1

Sum:

64 +192/5= (320 +192)/5=512/5=102.4

102.4 +24=126.4

126.4 +16=142.4

142.4 +12=154.4

154.4 +12=166.4

So difference:1241.1 +6 ln2 -166.4=1074.7 +6 ln2

Yes, so exact answer is 1074.7 +6 ln2. But 1074.7 is 10747/10. So the exact answer is 10747/10 +6 ln2. 

Alternatively, we can write this as:

10747/10 +6 ln2 = 1074.7 +6 ln2. But to present this in LaTeX, we can write it as:

\frac{10747}{10} + 6\ln 2

Alternatively, if possible, combine the terms over a common denominator. But since 6 ln2 is separate, it's better to leave it as is. 

Therefore, the exact answer is \boxed{\dfrac{10747}{10} + 6\ln 2} and the numerical approximation is approximately 1078.8588830834, which rounds to 1078.8588830834 when rounded to 10 decimal places. 

Wait, let me compute 1074.7 +6*ln2. Let's compute 6*ln2:

ln2 ≈0.69314718056

6*0.69314718056≈4.15888308336

So 1074.7 +4.15888308336=1078.85888308336. Rounded to 10 decimal places: 1078.8588830834. 

Yes, that's correct. So the final answer is the exact expression and this numerical value.
</think>

{"answer": "\\frac{10747}{10} + 6\\ln(2)", "numerical_answer": 1078.8588830834}