<think>
Okay, so I need to compute the definite integral from 0 to 2.0 of x^(1/2) times sin(1.0 times the fourth root of x(2.0 - x)) dx. Let me start by understanding the problem step by step.

First, the integrand is x^(1/2) sin(1.0 * (x(2 - x))^(1/4)). Let me write that more neatly: √x * sin( (x(2 - x))^{1/4} ). Hmm, the exponent 1/4 on the x(2 - x) term. That seems a bit complicated. Maybe there's a substitution that can simplify this expression.

Let me think about substitution. Let me set t = x(2 - x). Wait, but if I take t = x(2 - x), then dt/dx would be 2 - 2x. Hmm, but the integrand has sqrt(x) and the fourth root of t. Not sure if that helps directly. Alternatively, maybe a substitution inside the sine function. Let me see.

The argument of the sine is (x(2 - x))^{1/4}. Let me denote u = (x(2 - x))^{1/4}. Then u^4 = x(2 - x). Maybe differentiating u would give some relation. Let's try that. If u^4 = x(2 - x), then 4u^3 du/dx = 2 - 2x. Hmm, but I don't see an immediate way to express the integral in terms of u. The integrand is sqrt(x) sin(u), but sqrt(x) is x^{1/2}, which is part of the original variable. Maybe another substitution. Let's consider the entire expression under the fourth root. Let me set t = x(2 - x). Then, t = 2x - x^2. The derivative dt/dx = 2 - 2x. Hmm, but in the integrand, we have sqrt(x) sin(t^{1/4}). Not sure. Let's see if we can express sqrt(x) in terms of t. Since t = x(2 - x), maybe we can solve for x in terms of t, but that might be messy. Alternatively, perhaps a trigonometric substitution? Since the integrand has a sine function, maybe integrating by parts?

Integration by parts is a common technique. Let me recall that ∫u dv = uv - ∫v du. Let me set u_part = sin( (x(2 - x))^{1/4} ), and dv_part = x^{1/2} dx. Then du would be the derivative of the sine term, which is cos(...) times the derivative of the inside, and v would be the integral of x^{1/2}, which is (2/3)x^{3/2}. But this might complicate things because the derivative of the inside function (x(2 - x))^{1/4} would involve both x and (2 - x). Let me compute that derivative.

Let me denote f(x) = (x(2 - x))^{1/4}. Then f'(x) = (1/4)(x(2 - x))^{-3/4} * (2 - 2x). So f'(x) = (1/4)(x(2 - x))^{-3/4} * 2(1 - x) = (1/2)(1 - x)(x(2 - x))^{-3/4}. Hmm, so if I proceed with integration by parts, the new integral would involve cos(f(x)) times this derivative, multiplied by v, which is (2/3)x^{3/2}. That seems even more complicated. Maybe integration by parts isn't the way to go here.

Alternatively, maybe a substitution that can simplify the entire expression. Let me consider the substitution for the entire exponent. Let me set t = (x(2 - x))^{1/4}. Then t^4 = x(2 - x). Let me try to express x in terms of t. But solving for x from t^4 = 2x - x^2 would lead to a quadratic equation: x^2 - 2x + t^4 = 0. The solutions would be x = [2 ± sqrt(4 - 4t^4)] / 2 = 1 ± sqrt(1 - t^4). Hmm, but since x is between 0 and 2, maybe both solutions are valid? Let me check. For x in [0,2], t^4 = x(2 - x) which is a quadratic in x, peaking at x=1 with t^4=1. So t ranges from 0 to 1. When x=0, t=0; when x=2, t=0; at x=1, t=1. So t goes from 0 to 1 and back to 0. But if we take t as a variable, perhaps we can parametrize x in terms of t. However, this might split the integral into two parts: from 0 to 1 and 1 to 2, but maybe symmetry can help.

Wait, the original integral is from 0 to 2. Let me check if the integrand is symmetric around x=1. Let me substitute x = 2 - y. Then when x=0, y=2; x=2, y=0. The integrand becomes sqrt(2 - y) sin( ( (2 - y) y )^{1/4} ). Comparing to the original integrand sqrt(x) sin( (x(2 - x))^{1/4} ), which is sqrt(x) sin( (x(2 - x))^{1/4} ). So if we replace x with 2 - y, the argument of the sine is the same, but sqrt(2 - y) is sqrt(2 - y) instead of sqrt(y). So unless sqrt(x) and sqrt(2 - x) are symmetric in some way, maybe not. But perhaps there's a substitution that can exploit this.

Alternatively, maybe a substitution u = x - 1, shifting the interval to be symmetric around 0. Let u = x - 1, so x = u + 1. Then the integral becomes from u = -1 to u = 1. The integrand becomes sqrt(u + 1) sin( ( (u + 1)(1 - u) )^{1/4} ) du. The term (u + 1)(1 - u) is 1 - u^2, so the argument of the sine becomes (1 - u^2)^{1/4}. So the integrand is sqrt(u + 1) sin( (1 - u^2)^{1/4} ). Hmm, not sure if that helps. But maybe the function is even or odd. Let's check. If we replace u with -u, the integrand becomes sqrt(1 - u) sin( (1 - u^2)^{1/4} ). Which is different from the original, so not even. So symmetry might not help here.

Alternatively, perhaps a substitution that can turn the integral into a standard form. Let me think about the term inside the sine: (x(2 - x))^{1/4}. Let me set t = (x(2 - x))^{1/4}, so t^4 = x(2 - x). Then, as before, x^2 - 2x + t^4 = 0. Solving for x gives x = 1 ± sqrt(1 - t^4). But since x is between 0 and 2, and t is between 0 and 1, when t increases from 0 to 1, x moves from 1 to 1 (but actually, when t=0, x=0 or 2; when t=1, x=1). Wait, maybe this substitution is not injective over the interval. Because as x goes from 0 to 2, t goes from 0 up to 1 at x=1 and back to 0. So the substitution t = (x(2 - x))^{1/4} would require splitting the integral into two parts: from x=0 to x=1 (t from 0 to 1) and x=1 to x=2 (t from 1 back to 0). But integrating over t would then involve both branches. Maybe that's a way to proceed.

Let me try that. Let me split the integral into two parts: from 0 to 1 and from 1 to 2. Then, for each part, perform substitution t = (x(2 - x))^{1/4}. Let's first handle the interval from 0 to 1. Let t = (x(2 - x))^{1/4}, so t goes from 0 to 1 as x goes from 0 to 1. Then, t^4 = x(2 - x). Let me solve for x in terms of t. Rearranging, x^2 - 2x + t^4 = 0. Using quadratic formula: x = [2 ± sqrt(4 - 4t^4)] / 2 = 1 ± sqrt(1 - t^4). Since we're in the interval x from 0 to 1, we take the negative sign: x = 1 - sqrt(1 - t^4). Then, dx/dt = derivative of 1 - sqrt(1 - t^4) is (1/(2 sqrt(1 - t^4))) * 4t^3 = (2t^3)/sqrt(1 - t^4). So dx = (2t^3)/sqrt(1 - t^4) dt.

Now, for the integral from 0 to 1, substituting x = 1 - sqrt(1 - t^4), dx = (2t^3)/sqrt(1 - t^4) dt. The integrand sqrt(x) sin(t) becomes sqrt(1 - sqrt(1 - t^4)) * sin(t). Hmm, this seems complicated. Let me check sqrt(x): x = 1 - sqrt(1 - t^4), so sqrt(x) = sqrt(1 - sqrt(1 - t^4)). That's not a simple expression. Maybe this substitution isn't helpful.

Alternatively, perhaps another substitution. Let me think again. The integrand is sqrt(x) sin( (x(2 - x))^{1/4} ). Let me consider substituting u = x(2 - x). Then du = (2 - 2x) dx. But in the integrand, we have sqrt(x) sin(u^{1/4}) dx. Hmm, but we need to express sqrt(x) in terms of u and du. Let me see. If u = x(2 - x), then x(2 - x) = u. So x = [2 ± sqrt(4 - 4u)] / 2 = 1 ± sqrt(1 - u). But similar to before, this might split into two branches. However, maybe there's a way to express sqrt(x) in terms of u. Let's see. If u = x(2 - x), then 2x - x^2 = u. So x^2 - 2x + u = 0. Solving for x gives x = [2 ± sqrt(4 - 4u)] / 2 = 1 ± sqrt(1 - u). So sqrt(x) would be sqrt(1 ± sqrt(1 - u)). But this seems complicated again.

Alternatively, maybe a substitution that can make the argument of the sine function simpler. Let me set t = (x(2 - x))^{1/4}. Then, as before, t^4 = x(2 - x). Let me try to express sqrt(x) in terms of t. sqrt(x) = x^{1/2}. But x = [1 ± sqrt(1 - t^4)] as before. Hmm, not helpful.

Wait, maybe there's a substitution that combines both the sqrt(x) and the fourth root term. Let me think. Let me set t = x^{1/2}, so x = t^2, dx = 2t dt. Then the integral becomes from t=0 to t=sqrt(2). The integrand is t * sin( (t^2 (2 - t^2))^{1/4} ) * 2t dt = 2t^2 sin( (t^2 (2 - t^2))^{1/4} ) dt. Hmm, but the term inside the sine is (t^2 (2 - t^2))^{1/4} = (2t^2 - t^4)^{1/4}. Not sure if that helps. Maybe another substitution here. Let me set u = t^2, then du = 2t dt. But not sure.

Alternatively, maybe a substitution for the entire expression under the fourth root. Let me set v = t^2 (2 - t^2). Then dv/dt = 2t(2 - t^2) + t^2(-2t) = 4t - 2t^3 - 2t^3 = 4t - 4t^3. Hmm, but the integrand is 2t^2 sin(v^{1/4}) dt. Not sure.

This seems like a dead end. Maybe I need to consider that this integral doesn't have an elementary antiderivative. Let me check on Wolfram Alpha or another resource. Wait, but since I'm supposed to compute it analytically, maybe there's a trick I'm missing.

Wait, let me consider the substitution u = 1.0 * (x(2 - x))^{1/4}. Then, as before, u^4 = x(2 - x). Let me try to express x in terms of u. As before, x = 1 ± sqrt(1 - u^4). But maybe instead of splitting the integral, I can use symmetry. Let me check the original integrand. When x is replaced by 2 - x, the term x(2 - x) remains the same. So the argument of the sine function is symmetric around x=1. However, the sqrt(x) term becomes sqrt(2 - x). So the integrand is not symmetric. But maybe if I add the integral from 0 to 1 and from 1 to 2, there's a way to combine them.

Alternatively, perhaps a substitution that covers the entire interval. Let me set t = 1 - x. Then when x=0, t=1; x=2, t=-1. Not sure. Alternatively, maybe a trigonometric substitution. Let me think. Since x(2 - x) is similar to 1 - (x - 1)^2, which is a form of a circle equation. Let me check: x(2 - x) = 2x - x^2 = -(x^2 - 2x) = -(x^2 - 2x +1 -1) = -[(x -1)^2 -1] = 1 - (x -1)^2. So x(2 - x) = 1 - (x -1)^2. Therefore, the argument of the sine is [1 - (x -1)^2]^{1/4}. So the integrand becomes sqrt(x) sin( [1 - (x -1)^2]^{1/4} ). Hmm, maybe substituting x -1 = sinθ. Let me try that.

Let me set θ = arcsin(x -1). Then x = 1 + sinθ. Then dx = cosθ dθ. The limits of integration: when x=0, sinθ = -1, so θ = -π/2; when x=2, sinθ = 1, so θ = π/2. The integrand becomes sqrt(1 + sinθ) sin( [1 - sin^2θ]^{1/4} ). But 1 - sin^2θ = cos^2θ, so [1 - sin^2θ]^{1/4} = (cos^2θ)^{1/4} = cos^{1/2}θ. Therefore, the integrand becomes sqrt(1 + sinθ) sin( sqrt(cosθ) ). Hmm, this seems complicated. Also, sqrt(1 + sinθ) can be written as sqrt( (sin(θ/2) + cos(θ/2))^2 ) = |sin(θ/2) + cos(θ/2)|. But θ is between -π/2 and π/2, so θ/2 is between -π/4 and π/4, where sin(θ/2) + cos(θ/2) is positive. So sqrt(1 + sinθ) = sin(θ/2) + cos(θ/2). But even with that, the integrand becomes (sin(θ/2) + cos(θ/2)) * sin( sqrt(cosθ) ). This still doesn't look manageable. Maybe this substitution isn't helpful.

At this point, I'm starting to think that maybe this integral doesn't have an elementary antiderivative, and perhaps we need to resort to a series expansion or numerical integration. But the problem states to compute the integral analytically first. Hmm. Let me think again.

Wait, maybe expanding the sine function into its Taylor series. The integrand is sqrt(x) sin( (x(2 - x))^{1/4} ). Let me expand sin(z) as a power series: sin(z) = Σ_{n=0}^∞} (-1)^n z^{2n+1}/(2n+1)! ). So substituting z = (x(2 - x))^{1/4}, we get sin(z) = Σ (-1)^n (x(2 - x))^{(2n+1)/4} / (2n+1)! ). Then the integrand becomes sqrt(x) * Σ (-1)^n (x(2 - x))^{(2n+1)/4} / (2n+1)! ). So the integral becomes Σ (-1)^n / (2n+1)! ∫₀² x^{1/2} [x(2 - x)]^{(2n+1)/4} dx.

Let me simplify the exponent. x^{1/2} * [x(2 - x)]^{(2n+1)/4} = x^{1/2} * x^{(2n+1)/4} * (2 - x)^{(2n+1)/4} = x^{1/2 + (2n+1)/4} * (2 - x)^{(2n+1)/4}. Let me compute the exponent of x: 1/2 + (2n+1)/4 = (2 + 2n +1)/4 = (2n +3)/4. So the integral becomes Σ (-1)^n / (2n+1)! ∫₀² x^{(2n +3)/4} (2 - x)^{(2n +1)/4} dx.

This integral looks like a Beta function or a Gamma function integral. Recall that ∫₀² x^{a} (2 - x)^b dx = 2^{a + b +1} B(a+1, b+1) where B is the Beta function. Because substituting t = x/2, then x = 2t, dx = 2dt, and the integral becomes ∫₀¹ (2t)^a (2 - 2t)^b 2 dt = 2^{a + b +1} ∫₀¹ t^a (1 - t)^b dt = 2^{a + b +1} B(a+1, b+1). And B(a+1, b+1) = Γ(a+1)Γ(b+1)/Γ(a + b + 2).

So applying this to our case, a = (2n +3)/4, b = (2n +1)/4. Then the integral becomes 2^{a + b +1} B(a+1, b+1) = 2^{( (2n +3)/4 + (2n +1)/4 ) +1} B( (2n +3)/4 +1, (2n +1)/4 +1 ). Let's compute the exponent: (2n +3 + 2n +1)/4 +1 = (4n +4)/4 +1 = (n +1) +1 = n +2. So 2^{n +2} B( (2n +7)/4, (2n +5)/4 ). Then, using the Beta function in terms of Gamma functions: B(p, q) = Γ(p)Γ(q)/Γ(p + q). So the integral becomes 2^{n +2} Γ( (2n +7)/4 ) Γ( (2n +5)/4 ) / Γ( (2n +7)/4 + (2n +5)/4 ) = 2^{n +2} Γ( (2n +7)/4 ) Γ( (2n +5)/4 ) / Γ( (4n +12)/4 ) = 2^{n +2} Γ( (2n +7)/4 ) Γ( (2n +5)/4 ) / Γ( n +3 ).

But Γ(n +3) is (n +2)! So the integral is 2^{n +2} Γ( (2n +7)/4 ) Γ( (2n +5)/4 ) / (n +2)!.

Hmm, this seems complicated, but maybe there's a simplification. Let me recall the duplication formula for Gamma functions: Γ(z)Γ(z + 1/2) = 2^{1 - 2z} sqrt(π) Γ(2z). Let me check if the product Γ( (2n +5)/4 ) Γ( (2n +7)/4 ) can be expressed using the duplication formula. Let me set z = (2n +5)/4. Then z + 1/2 = (2n +5)/4 + 2/4 = (2n +7)/4. So Γ(z)Γ(z + 1/2) = Γ( (2n +5)/4 ) Γ( (2n +7)/4 ) = 2^{1 - 2z} sqrt(π) Γ(2z). Substituting z = (2n +5)/4, we get 2^{1 - 2*(2n +5)/4} sqrt(π) Γ(2*(2n +5)/4) = 2^{1 - (2n +5)/2} sqrt(π) Γ( (2n +5)/2 ). Simplifying the exponent: 1 - (2n +5)/2 = (2 - 2n -5)/2 = (-2n -3)/2 = - (2n +3)/2. So 2^{-(2n +3)/2} sqrt(π) Γ( (2n +5)/2 ). Therefore, Γ( (2n +5)/4 ) Γ( (2n +7)/4 ) = 2^{-(2n +3)/2} sqrt(π) Γ( (2n +5)/2 ).

Substituting back into the integral expression, we have:

Integral = 2^{n +2} * [2^{-(2n +3)/2} sqrt(π) Γ( (2n +5)/2 ) ] / (n +2)! )

Simplify the exponents: 2^{n +2} * 2^{ - (2n +3)/2 } = 2^{n +2 - (2n +3)/2} = 2^{(2n +4 -2n -3)/2} = 2^{(1)/2} = sqrt(2). So the integral becomes sqrt(2) sqrt(π) Γ( (2n +5)/2 ) / (n +2)! )

Therefore, the integral over [0,2] of x^{1/2} sin( (x(2 -x))^{1/4} ) dx is equal to the sum from n=0 to infinity of (-1)^n / (2n +1)! * sqrt(2) sqrt(π) Γ( (2n +5)/2 ) / (n +2)! )

Hmm, this seems challenging. Let me see if Γ( (2n +5)/2 ) can be expressed in terms of factorials or other Gamma functions. Recall that Γ(k + 1/2) for integer k can be expressed as (2k)! sqrt(π)/(4^k k!)). But (2n +5)/2 = n + 5/2. So Γ(n + 5/2) = Γ( (2n +5)/2 ). For example, Γ(5/2) = (3/2)(1/2) sqrt(π) = (3/4) sqrt(π). Γ(7/2) = (5/2)(3/2)(1/2) sqrt(π) = (15/8) sqrt(π), etc. In general, Γ(n + 5/2) = ( (2n +3)!! ) / 2^{n +2} ) sqrt(π). Where (2n +3)!! is the double factorial: (2n +3)(2n +1)...5*3*1.

So Γ( (2n +5)/2 ) = Γ(n + 5/2) = (2n +3)!! / 2^{n +2} sqrt(π). Therefore, substituting back into the integral expression:

Integral = sum_{n=0}^∞ (-1)^n / (2n +1)! * sqrt(2) sqrt(π) * [ (2n +3)!! / 2^{n +2} sqrt(π) ] / (n +2)! )

Simplify this expression:

sqrt(2) sqrt(π) * [ (2n +3)!! / 2^{n +2} sqrt(π) ] = sqrt(2) * (2n +3)!! / 2^{n +2} = (2n +3)!! / (2^{n +2} / sqrt(2)) ) = (2n +3)!! / (2^{n + 3/2} )

So the integral becomes sum_{n=0}^∞ (-1)^n / (2n +1)! * (2n +3)!! / (2^{n + 3/2} (n +2)! ) )

Hmm, this is getting quite involved. Let me see if I can simplify the terms. Note that (2n +3)!! = (2n +3)(2n +1)...5*3*1. Also, (2n +1)! = (2n +1)(2n)...2*1. There might be a relationship between (2n +3)!! and (2n +1)!.

Alternatively, note that (2n +3)!! = (2n +3)! / (2^{n +1} (n +1)! ) ). Because (2n +3)! = (2n +3)(2n +2)(2n +1)...2*1. The double factorial (2n +3)!! is the product of the odd numbers up to 2n +3. So (2n +3)!! = (2n +3)! / (2^{n +1} (n +1)! ) ). Let me verify for n=0: (0 +3)!! = 3!! = 3*1 = 3. (2*0 +3)! = 3! = 6. 2^{0 +1} (0 +1)! = 2*1 = 2. 6 / 2 = 3. Correct. For n=1: (2*1 +3)!! =5!!=5*3*1=15. (2*1 +3)! =5!=120. 2^{1+1}(1+1)! =4*2=8. 120/8=15. Correct. So yes, (2n +3)!! = (2n +3)! / (2^{n +1} (n +1)! ) ).

Substituting this into the expression:

Integral = sum_{n=0}^∞ (-1)^n / (2n +1)! * [ (2n +3)! / (2^{n +1} (n +1)! ) ) ] / (2^{n + 3/2} (n +2)! ) )

Simplify the denominators:

Denominator terms: 2^{n +1} (n +1)! * 2^{n + 3/2} (n +2)! = 2^{2n + 5/2} (n +1)! (n +2)! )

Numerator: (2n +3)! 

So the term becomes:

(2n +3)! / [2^{2n +5/2} (n +1)! (n +2)! (2n +1)! ) ] * (-1)^n

Wait, but the original term is [ (2n +3)!! ] / [ 2^{n +3/2} (n +2)! ) ] * (-1)^n / (2n +1)! )

But substituting (2n +3)!! = (2n +3)! / (2^{n +1} (n +1)! ), we get:

[ (2n +3)! / (2^{n +1} (n +1)! ) ] / [2^{n +3/2} (n +2)! ) ] * (-1)^n / (2n +1)! )

= (2n +3)! / [2^{n +1} (n +1)! * 2^{n +3/2} (n +2)! ) ] * (-1)^n / (2n +1)! )

= (2n +3)! / [2^{2n +5/2} (n +1)! (n +2)! ) ] * (-1)^n / (2n +1)! )

But (2n +3)! / (2n +1)! ) = (2n +3)(2n +2)

So this becomes:

(2n +3)(2n +2) / [2^{2n +5/2} (n +1)! (n +2)! ) ] * (-1)^n

Simplify (2n +3)(2n +2) = 2(n +1)(2n +3)

So:

2(n +1)(2n +3) / [2^{2n +5/2} (n +1)! (n +2)! ) ] * (-1)^n

Cancel (n +1) in numerator and denominator:

2(2n +3) / [2^{2n +5/2} (n +2)! ) ] * (-1)^n

Note that (n +2)! = (n +2)(n +1)! but we already canceled (n +1). Wait, no, (n +2)! = (n +2)(n +1)!

But in the denominator, after canceling (n +1)!, we have (n +2)! = (n +2)(n +1)! ), but we already canceled one (n +1)!.

Wait, let me re-express:

Original denominator after substitution: 2^{2n +5/2} (n +1)! (n +2)! )

After substituting (2n +3)!! and simplifying, we have:

(2n +3)(2n +2) / [2^{2n +5/2} (n +1)! (n +2)! ) ] * (-1)^n / (2n +1)! )

Wait, perhaps I made a mistake in the simplification steps. Let me start over.

After substituting (2n +3)!! = (2n +3)! / (2^{n +1} (n +1)! ), the term becomes:

Integral term = [ (2n +3)! / (2^{n +1} (n +1)! ) ] / [2^{n +3/2} (n +2)! ) ] * (-1)^n / (2n +1)! )

= (2n +3)! / [2^{n +1} (n +1)! * 2^{n +3/2} (n +2)! ) ] * (-1)^n / (2n +1)! )

= (2n +3)! / [2^{2n +5/2} (n +1)! (n +2)! ) ] * (-1)^n / (2n +1)! )

Now, (2n +3)! / (2n +1)! ) = (2n +3)(2n +2)

So:

= (2n +3)(2n +2) / [2^{2n +5/2} (n +1)! (n +2)! ) ] * (-1)^n

Factor out 2 from (2n +2):

= 2(n +1)(2n +3) / [2^{2n +5/2} (n +1)! (n +2)! ) ] * (-1)^n

Cancel (n +1) in numerator and denominator:

= 2(2n +3) / [2^{2n +5/2} (n +2)! ) ] * (-1)^n

Simplify 2 / 2^{2n +5/2} = 2^{1 -2n -5/2} = 2^{-2n -3/2}

So:

= (2n +3) * 2^{-2n -3/2} / (n +2)! ) * (-1)^n

Therefore, the integral term becomes:

(-1)^n (2n +3) / (2^{2n +3/2} (n +2)! )

So the entire integral is the sum from n=0 to ∞ of [ (-1)^n (2n +3) ] / [2^{2n +3/2} (n +2)! ) ]

Hmm, this is still a complicated series, but perhaps it can be expressed in terms of known functions. Let me see if I can relate this to a Taylor series of some function.

Let me factor out 1/2^{3/2} from the sum:

Integral = (1 / 2^{3/2}) Σ_{n=0}^∞ (-1)^n (2n +3) / (2^{2n} (n +2)! )

Let me make a substitution m = n +2. Then when n=0, m=2. So:

Σ_{n=0}^∞ (-1)^n (2n +3) / (2^{2n} (n +2)! ) = Σ_{m=2}^∞ (-1)^{m-2} (2(m-2) +3) / (2^{2(m-2)} (m)! ) )

Simplify the terms:

2(m -2) +3 = 2m -4 +3 = 2m -1

(-1)^{m -2} = (-1)^m (-1)^{-2} = (-1)^m

So the sum becomes Σ_{m=2}^∞ (-1)^m (2m -1) / (2^{2m -4} m! )

But 2^{2m -4} = 2^{2m} / 16. So:

Σ_{m=2}^∞ (-1)^m (2m -1) * 16 / (2^{2m} m! ) = 16 Σ_{m=2}^∞ (-1)^m (2m -1) / (4^m m! )

= 16 Σ_{m=2}^∞ (-1)^m (2m -1) / (4^m m! )

But this seems like it could be related to the series expansion of e^{-1/4} or something similar, but I'm not sure. Let me consider expanding e^{-x} and see if the terms match.

The Taylor series for e^{-x} is Σ_{k=0}^∞ (-x)^k /k! = Σ_{k=0}^∞ (-1)^k x^k /k!.

But our sum involves terms like (2m -1)/4^m m! for m >=2. Let me consider differentiating or integrating the series for e^{-x} to see if I can generate such terms.

Let me set x = 1/4. Then e^{-1/4} = Σ_{k=0}^∞ (-1)^k (1/4)^k /k! = Σ_{k=0}^∞ (-1)^k / (4^k k! )

But our sum is Σ_{m=2}^∞ (-1)^m (2m -1) / (4^m m! ). Let me write this as Σ_{m=2}^∞ (-1)^m (2m -1) / (4^m m! ) = Σ_{m=2}^∞ [2m /4^m m! - 1/4^m m! ] (-1)^m = 2 Σ_{m=2}^∞ (-1)^m m / (4^m m! ) - Σ_{m=2}^∞ (-1)^m / (4^m m! )

Let me handle each sum separately.

First sum: 2 Σ_{m=2}^∞ (-1)^m m / (4^m m! ) = 2 Σ_{m=2}^∞ (-1)^m / (4^m (m-1)! )

Because m/m! = 1/(m-1)!.

Similarly, the second sum: - Σ_{m=2}^∞ (-1)^m / (4^m m! )

Let me adjust the indices. For the first sum, let k = m -1. Then when m=2, k=1. So:

2 Σ_{k=1}^∞ (-1)^{k+1} / (4^{k+1} k! ) = 2 * (-1) Σ_{k=1}^∞ (-1)^k / (4^{k+1} k! ) = -2/4 Σ_{k=1}^∞ (-1)^k / (4^k k! ) = -1/2 [ Σ_{k=1}^∞ (-1)^k / (4^k k! ) ]

Similarly, the second sum: - Σ_{m=2}^∞ (-1)^m / (4^m m! ) = - [ Σ_{m=0}^∞ (-1)^m / (4^m m! ) - 1 + 1/4 ]

Because Σ_{m=0}^∞ (-1)^m / (4^m m! ) = e^{-1/4}, so subtracting the first two terms (m=0 and m=1) gives Σ_{m=2}^∞.

So:

Second sum = - [ e^{-1/4} - 1 + 1/4 ] = -e^{-1/4} + 1 - 1/4 = -e^{-1/4} + 3/4.

Putting it all together:

Original sum = first sum + second sum = -1/2 [ Σ_{k=1}^∞ (-1)^k / (4^k k! ) ] + (-e^{-1/4} + 3/4 )

But Σ_{k=1}^∞ (-1)^k / (4^k k! ) = e^{-1/4} - 1. Because Σ_{k=0}^∞ (-1)^k / (4^k k! ) = e^{-1/4}, so subtract the k=0 term (1) to get the sum from k=1.

Therefore:

First sum = -1/2 (e^{-1/4} -1 )

Second sum = -e^{-1/4} + 3/4

So total sum = -1/2 e^{-1/4} + 1/2 - e^{-1/4} + 3/4 = (-1/2 -1) e^{-1/4} + (1/2 + 3/4 ) = -3/2 e^{-1/4} + 5/4

Therefore, the original sum is -3/2 e^{-1/4} + 5/4.

But recall that the integral was (1 / 2^{3/2}) times this sum. So Integral = (1 / 2^{3/2}) * ( -3/2 e^{-1/4} + 5/4 ) = (1 / (2*sqrt(2))) * ( -3/2 e^{-1/4} + 5/4 )

Simplify:

= (1 / (2*sqrt(2))) * ( (5/4) - (3/2) e^{-1/4} )

= (5/(8 sqrt(2)) ) - (3/(4 sqrt(2)) ) e^{-1/4}

Rationalizing the denominators:

5/(8 sqrt(2)) = 5 sqrt(2)/16

3/(4 sqrt(2)) = 3 sqrt(2)/8

So Integral = (5 sqrt(2)/16) - (3 sqrt(2)/8) e^{-1/4}

Factor out sqrt(2)/16:

= sqrt(2)/16 (5 - 6 e^{-1/4} )

Therefore, the exact value of the integral is sqrt(2)/16 (5 - 6 e^{-1/4} )

Let me verify this result. Let's compute e^{-1/4} ≈ e^{-0.25} ≈ 0.7788007831.

So 5 -6*0.7788007831 ≈5 -4.6728047 ≈0.3271953

Then sqrt(2)/16 ≈0.0883883476

Multiply: 0.0883883476 *0.3271953 ≈0.0289. Let me check with a numerical approximation. Let me compute the integral numerically to see if it's approximately 0.0289.

Alternatively, let me compute the numerical value of the exact expression:

sqrt(2)/16*(5 -6*exp(-1/4)).

Compute each part:

sqrt(2) ≈1.41421356237

1/4 =0.25

exp(-0.25) ≈0.7788007830714049

5 -6*0.7788007830714049 =5 -4.672804698428429=0.327195301571571

sqrt(2)/16 ≈1.41421356237 /16 ≈0.088388347648318

Multiply: 0.088388347648318 *0.327195301571571 ≈0.0289.

Now, let me compute the integral numerically using a calculator or approximate method. Let's use Simpson's rule with a few intervals to estimate.

The integral is from 0 to 2 of sqrt(x) sin( (x(2 -x))^{1/4} ) dx.

Let me approximate this using numerical integration method. Let's use x from 0 to 2. Let's split into, say, 4 intervals. But for better accuracy, maybe use more intervals. Alternatively, use an online integral calculator.

Alternatively, use Python code to compute it numerically. But since I can't run code here, let me estimate.

Alternatively, check if the exact answer I derived matches the numerical approximation. The exact answer is sqrt(2)/16*(5 -6*exp(-1/4)) ≈0.0289. Let me compute this more precisely.

Compute sqrt(2) ≈1.41421356237

exp(-0.25) ≈0.7788007830714049

5 -6*0.7788007830714049 =5 -4.672804698428429=0.327195301571571

sqrt(2)/16=1.41421356237 /16=0.088388347648318

Multiply: 0.088388347648318 *0.327195301571571=0.0883883476 *0.3271953016 ≈0.028903

So the exact value is approximately 0.028903. Let me check with a numerical approximation.

Alternatively, use substitution to check. Let me use substitution x = t^2, then dx=2t dt. The integral becomes ∫0^sqrt(2) t * sin( (t^2 (2 - t^2))^{1/4} ) * 2t dt = 2 ∫0^{sqrt(2)} t^2 sin( (t^2 (2 - t^2))^{1/4} ) dt. Let me approximate this integral numerically.

But without computational tools, it's hard, but given that the exact answer is approximately 0.0289, and the steps seem correct, I think this is the correct analytical result.

Therefore, the exact answer is sqrt(2)/16 (5 -6 e^{-1/4} ), and the numerical approximation is approximately 0.028903, which rounds to 0.028903 when rounded to 10 decimal places. Let me compute it precisely:

Compute 5 -6*exp(-1/4):

exp(-0.25) = e^{-0.25} ≈0.7788007830714049

6*0.7788007830714049=4.672804698428429

5 -4.672804698428429=0.327195301571571

Multiply by sqrt(2)/16:

sqrt(2)=1.4142135623730951

sqrt(2)/16=0.08838834764831845

0.08838834764831845 *0.327195301571571=0.02890293901

Rounded to 10 decimal places: 0.0289029390

So the numerical approximation is approximately 0.0289029390.
</think>

{"answer": "\\dfrac{\\sqrt{2}}{16} \\left(5 - 6e^{-1/4}\\right)", "numerical_answer": "0.0289029390"}