Let's proceed step by step:

**Step 1: Find the antiderivative analytically.**

The integrand is:
\[
f(x) = x^5 + 5x^4 + 10x^3 + 8x^2 + x
\]

Integrate term by term:
\[
\int f(x) \, dx = \int \left( x^5 + 5x^4 + 10x^3 + 8x^2 + x \right) \, dx
\]
\[
= \frac{x^6}{6} + 5\frac{x^5}{5} + 10\frac{x^4}{4} + 8\frac{x^3}{3} + \frac{x^2}{2}
\]
\[
= \frac{x^6}{6} + x^5 + \frac{5x^4}{2} + \frac{8x^3}{3} + \frac{x^2}{2}
\]

**Step 2: Evaluate from \( x = -\frac{3}{2} \) to \( x = -\frac{1}{2} \).**

Set
\[
F(x) = \frac{x^6}{6} + x^5 + \frac{5x^4}{2} + \frac{8x^3}{3} + \frac{x^2}{2}
\]
We want
\[
F\left(-\frac{1}{2}\right) - F\left(-\frac{3}{2}\right)
\]

First, calculate \( F\left(-\frac{1}{2}\right) \):

- \(x = -\frac{1}{2}\)

1. \(x^2 = \frac{1}{4} \)
2. \(x^3 = -\frac{1}{8}\)
3. \(x^4 = \frac{1}{16}\)
4. \(x^5 = -\frac{1}{32}\)
5. \(x^6 = \frac{1}{64}\)

So,
\[
F\left(-\frac{1}{2}\right) = \frac{1}{64} \cdot \frac{1}{6} - \frac{1}{32} + \frac{5}{2} \cdot \frac{1}{16} + \frac{8}{3} \cdot \left(-\frac{1}{8}\right) + \frac{1}{2} \cdot \frac{1}{4}
\]
\[
= \frac{1}{384} - \frac{1}{32} + \frac{5}{32} - \frac{1}{3} + \frac{1}{8}
\]

Let’s write all with common denominator 384:

- \(\frac{1}{384}\)
- \(-\frac{1}{32} = -\frac{12}{384}\)
- \(\frac{5}{32} = \frac{60}{384}\)
- \(-\frac{1}{3} = -\frac{128}{384}\)
- \(\frac{1}{8} = \frac{48}{384}\)

Combine:
\[
\frac{1 - 12 + 60 - 128 + 48}{384} = \frac{(1 + 60 + 48) - (12 + 128)}{384}
\]
\[
= \frac{(109) - (140)}{384} = \frac{-31}{384}
\]

**So:** \( F\left(-\frac{1}{2}\right) = -\frac{31}{384} \)

---

Now for \( F\left(-\frac{3}{2}\right) \):

- \(x = -\frac{3}{2}\)

1. \( x^2 = \left(\frac{9}{4}\right) \)
2. \( x^3 = -\frac{27}{8} \)
3. \( x^4 = \frac{81}{16} \)
4. \( x^5 = -\frac{243}{32} \)
5. \( x^6 = \frac{729}{64} \)

Plug in:
\[
F\left(-\frac{3}{2}\right) = \frac{729}{64 \cdot 6} + \left(-\frac{243}{32}\right) + \frac{5}{2} \cdot \frac{81}{16} + \frac{8}{3} \cdot \left(-\frac{27}{8}\right) + \frac{1}{2} \cdot \frac{9}{4}
\]

Let’s compute each term:
- \( \frac{729}{384} \)
- \( -\frac{243}{32} \)
- \( \frac{5 \cdot 81}{32} = \frac{405}{32} \)
- \( -\frac{27}{3} = -9 \)
- \( \frac{9}{8} \)

Combine all terms with denominator 384:
- \( \frac{729}{384} \)
- \( -\frac{243}{32} = -\frac{2916}{384} \)
- \( \frac{405}{32} = \frac{4860}{384} \)
- \( -9 = -\frac{3456}{384} \)
- \( \frac{9}{8} = \frac{432}{384} \)

Sum:
\[
729 - 2916 + 4860 - 3456 + 432 = (729 + 4860 + 432) - (2916 + 3456) = (6021) - (6372) = -351
\]
So,
\[
F\left(-\frac{3}{2}\right) = \frac{-351}{384}
\]

**Compute the definite integral:**
\[
F\left(-\frac{1}{2}\right) - F\left(-\frac{3}{2}\right) = \left(-\frac{31}{384}\right) - \left(-\frac{351}{384}\right) = \frac{320}{384} = \frac{5}{6}
\]

**Step 3: Numerical approximation**

\[
\frac{5}{6} \approx 0.8333333333
\]

**Step 4: JSON output**

```json
{"answer": "\\frac{5}{6}", "numerical_answer": "0.8333333333"}
```