# Evaluating $\int_{-1}^1 x^2 \cdot \sqrt[3]{x^3+1} \, dx$

I'll solve this integral using a substitution approach.

## Step 1: Make a substitution
Let's use $u = x^3 + 1$, which means:
- $du = 3x^2 \, dx$
- $x^2 \, dx = \frac{du}{3}$

When $x = -1$, $u = (-1)^3 + 1 = -1 + 1 = 0$
When $x = 1$, $u = 1^3 + 1 = 1 + 1 = 2$

## Step 2: Rewrite the integral in terms of $u$
$\int_{-1}^1 x^2 \cdot \sqrt[3]{x^3+1} \, dx = \int_{-1}^1 x^2 \cdot (x^3+1)^{1/3} \, dx$

Using our substitution:
$\int_{-1}^1 x^2 \cdot (x^3+1)^{1/3} \, dx = \int_{0}^{2} \frac{1}{3} \cdot u^{1/3} \, du$

## Step 3: Evaluate the integral
$\int_{0}^{2} \frac{1}{3} \cdot u^{1/3} \, du = \frac{1}{3} \int_{0}^{2} u^{1/3} \, du$

Using the power rule: $\int u^n \, du = \frac{u^{n+1}}{n+1} + C$ for $n \neq -1$

For our integral, $n = 1/3$, so:
$\frac{1}{3} \int_{0}^{2} u^{1/3} \, du = \frac{1}{3} \cdot \frac{u^{4/3}}{4/3} \bigg|_{0}^{2} = \frac{1}{4} u^{4/3} \bigg|_{0}^{2}$

Evaluating at the bounds:
$\frac{1}{4} u^{4/3} \bigg|_{0}^{2} = \frac{1}{4} \cdot 2^{4/3} - \frac{1}{4} \cdot 0^{4/3} = \frac{1}{4} \cdot 2^{4/3} = \frac{2^{4/3}}{4}$

We can simplify this:
$\frac{2^{4/3}}{4} = \frac{2^{4/3}}{2^2} = 2^{4/3-2} = 2^{4/3-6/3} = 2^{-2/3}$

## Step 4: Final exact answer
The exact answer is $2^{-2/3}$ or $\frac{1}{2^{2/3}}$

## Step 5: Numerical approximation
$2^{-2/3} \approx 0.6299605249$

{"answer": "2^{-2/3}", "numerical_answer": "0.6299605249"}