We start with the integral

  I = ∫₀¹ [ln(1 + x + x²)]/x dx.

Step 1. Rewrite ln(1 + x + x²) in a more convenient form.

Notice that
  1 + x + x² = (1 − x³)/(1 − x)   (for x ≠ 1),
since
  (1 − x)(1 + x + x²) = 1 − x³.
Taking logarithms we have
  ln(1 + x + x²) = ln(1 − x³) − ln(1 − x).

Thus, the integral becomes
  I = ∫₀¹ [1/x] [ln(1 − x³) − ln(1 − x)] dx.

Step 2. Expand the logarithms in power series.

Recall the Taylor expansion (for |x| < 1):
  ln(1 − u) = −∑ₙ₌₁∞ (uⁿ/n).

• For u = x³:
  ln(1 − x³) = −∑ₙ₌₁∞ (x^(3n)/n).

• For u = x:
  ln(1 − x) = −∑ₙ₌₁∞ (xⁿ/n).

Taking the difference,
  ln(1 − x³) − ln(1 − x) = −∑ₙ₌₁∞ (x^(3n)/n) + ∑ₙ₌₁∞ (xⁿ/n)
                 = ∑ₙ₌₁∞ [xⁿ − x^(3n)]/n.

Step 3. Substitute the series back into the integral.

We now have
  I = ∫₀¹ [1/x] ∑ₙ₌₁∞ [xⁿ − x^(3n)]/n dx.
Interchange the order of summation and integration (this is justified by uniform convergence on [0,1)) to obtain
  I = ∑ₙ₌₁∞ (1/n) ∫₀¹ [xⁿ − x^(3n)]/x dx
    = ∑ₙ₌₁∞ (1/n) ∫₀¹ [x^(n−1) − x^(3n−1)] dx.

Step 4. Evaluate the integrals term‐by‐term.

For α > 0,
  ∫₀¹ x^(α−1) dx = 1/α.
Thus,
  ∫₀¹ x^(n−1) dx = 1/n   and  ∫₀¹ x^(3n−1) dx = 1/(3n).

So the n‑th term contributes
  (1/n)[1/n − 1/(3n)] = (1/n) (1 − 1/3)/n = (1/n)(2/(3n)) = 2/(3n²).

Then
  I = ∑ₙ₌₁∞ 2/(3n²) = (2/3) ∑ₙ₌₁∞ 1/n².

Step 5. Recognize the sum as the Riemann zeta function.

We have
  ∑ₙ₌₁∞ 1/n² = ζ(2) = π²/6.
Thus,
  I = (2/3)(π²/6) = π²/9.

Step 6. Provide the numerical approximation.

We have
  π²/9 ≈ (9.869604401089358)/9 ≈ 1.0966227112.

The final answer in the required JSON format is:
{"answer": "\\frac{\\pi^2}{9}", "numerical_answer": "1.0966227112"}