<think>
Okay, let's tackle this integral step by step. The problem is to compute the definite integral from 1 to 2 of 2^{x-1} + log base 2 of (2x) dx. Alright, first, I need to break this into two separate integrals because the integral of a sum is the sum of the integrals. So, I can write it as the integral of 2^{x-1} dx plus the integral of log_2(2x) dx, both from 1 to 2.

Starting with the first part: the integral of 2^{x-1} dx. I remember that the integral of a^u du is a^u / ln(a) + C. Here, the base is 2, and the exponent is x-1. Let me make sure. If I let u = x-1, then du = dx. So the integral becomes 2^u du, which is 2^u / ln(2) + C. Substituting back, that's 2^{x-1} / ln(2). So evaluated from 1 to 2, that would be [2^{2-1}/ln(2)] - [2^{1-1}/ln(2)] = (2^1 / ln(2)) - (2^0 / ln(2)) = (2/ln(2)) - (1/ln(2)) = (2 - 1)/ln(2) = 1/ln(2). Okay, that's the first part.

Now the second integral: integral of log_2(2x) dx from 1 to 2. Hmm, log base 2 can be tricky. Maybe I can simplify the logarithm first. Remember that log_2(2x) is the same as log_2(2) + log_2(x), right? Because log_b(ab) = log_b a + log_b b. So log_2(2x) = log_2(2) + log_2(x) = 1 + log_2(x). So the integral becomes the integral of 1 dx plus the integral of log_2(x) dx, from 1 to 2.

The integral of 1 dx from 1 to 2 is straightforward. That's just x evaluated from 1 to 2, which is 2 - 1 = 1.

Now the integral of log_2(x) dx. To integrate log base 2 of x, I can convert it to natural logarithm. Since log_2(x) = ln(x)/ln(2). So the integral becomes (1/ln(2)) integral of ln(x) dx. The integral of ln(x) dx is x ln(x) - x + C. So putting it all together, the integral of log_2(x) dx is (1/ln(2))(x ln(x) - x) evaluated from 1 to 2.

Let's compute that. At x=2: (2 ln(2) - 2). At x=1: (1 ln(1) - 1) = (0 - 1) = -1. So subtracting, we get [2 ln(2) - 2 - (-1)] = 2 ln(2) - 1. Then multiply by 1/ln(2): (2 ln(2) - 1)/ln(2) = 2 - 1/ln(2).

Wait, let me check that again. Let me compute the definite integral:

(1/ln(2)) [ (2 ln 2 - 2) - (1 ln 1 -1) ] = (1/ln(2)) [ (2 ln 2 - 2) - (0 -1) ] = (1/ln(2)) [2 ln 2 -2 +1] = (1/ln(2))(2 ln 2 -1). Hmm, so that's (2 ln 2 -1)/ln(2). Which can be written as 2 - (1/ln(2)). Wait, 2 ln2 / ln2 is 2, and -1/ln2. So yes, 2 - 1/ln2. So the integral of log_2(x) from 1 to 2 is 2 - 1/ln2.

But wait, the original integral for the second part was log_2(2x), which we split into 1 + log_2(x). So the integral of log_2(2x) dx from 1 to 2 is the integral of 1 dx (which is 1) plus the integral of log_2(x) dx (which is 2 - 1/ln2). So total is 1 + 2 - 1/ln2 = 3 - 1/ln2.

Wait, let me verify that again. The integral of log_2(2x) dx from 1 to 2 is equal to integral of 1 dx (from 1 to 2) which is 1, plus integral of log_2(x) dx from 1 to 2. The integral of log_2(x) dx from 1 to 2 is (1/ln2)(x lnx -x) evaluated from 1 to 2. At 2: 2 ln2 -2. At 1: 1*0 -1 = -1. So (2 ln2 -2) - (-1) = 2 ln2 -1. Multiply by 1/ln2: (2 ln2 -1)/ln2 = 2 - 1/ln2. So the integral of log_2(x) is 2 -1/ln2, so adding the 1 from the 1 dx part, total is 3 -1/ln2.

So combining both parts: the first integral was 1/ln2, the second integral is 3 -1/ln2. So total integral is 1/ln2 + 3 -1/ln2 = 3. Wait, that's interesting. The 1/ln2 and -1/ln2 cancel each other, leaving 3. But that seems too simple. Let me check again.

First integral: ∫1^2 2^{x-1} dx = 1/ln2.

Second integral: ∫1^2 log2(2x) dx = 3 -1/ln2.

Adding them together: 1/ln2 + 3 -1/ln2 = 3. So the exact answer is 3? That's surprising. Let me confirm.

Wait, maybe I made a mistake in splitting the log. Let's re-examine log_2(2x). Yes, log_2(2x) = log_2(2 + log_2 x) = 1 + log_2 x. So the integral is ∫1^2 [1 + log2 x] dx = ∫1^2 1 dx + ∫1^2 log2 x dx. The first part is 1*(2-1)=1. The second part is ∫1^2 log2 x dx. As we computed, that's 2 -1/ln2. So total is 1 + 2 -1/ln2 = 3 -1/ln2. Wait, but then adding the first integral's result, which is 1/ln2, so total integral is 1/ln2 + 3 -1/ln2 = 3. So the exact answer is 3? That's possible? Let me check with numerical approximation.

Alternatively, maybe I made a mistake in the integration steps. Let's verify each step again.

First integral: ∫2^{x-1} dx. Let u = x-1, du=dx. So ∫2^u du = 2^u / ln2 + C. Evaluated from 1 to 2: at x=2, u=1: 2^1 / ln2 = 2/ln2. At x=1, u=0: 2^0 / ln2 = 1/ln2. So difference is (2 -1)/ln2 = 1/ln2. Correct.

Second integral: ∫log2(2x) dx. Split into 1 + log2 x. Integral of 1 from 1 to 2 is 1. Integral of log2 x from 1 to 2. As before, using integration by parts. Let u = log2 x, dv = dx. Then du = (1/(x ln2)) dx, v = x. So ∫log2 x dx = x log2 x - ∫x*(1/(x ln2)) dx = x log2 x - ∫1/ln2 dx = x log2 x - x/ln2 + C. Evaluated from 1 to 2.

At x=2: 2 log2 2 - 2/ln2. Since log2 2 =1, so 2*1 - 2/ln2 = 2 - 2/ln2.

At x=1: 1 log2 1 -1/ln2. log2 1=0, so 0 -1/ln2 = -1/ln2.

Subtracting: (2 -2/ln2) - (-1/ln2) = 2 -2/ln2 +1/ln2 = 2 -1/ln2.

So the integral of log2 x from 1 to 2 is 2 -1/ln2. Then adding the 1 from the first part, total is 1 + (2 -1/ln2) = 3 -1/ln2. Wait, no. Wait, the integral of log2(2x) is ∫1 dx (which is 1) + ∫log2 x dx (which is 2 -1/ln2). So total is 1 + 2 -1/ln2 = 3 -1/ln2. Then adding the first integral's result, which is 1/ln2, the total integral is 1/ln2 +3 -1/ln2 =3. So the exact answer is 3. That's correct? Let me check with a numerical approximation.

Alternatively, maybe there's a simpler way. Let's compute the entire integral:

∫1^2 [2^{x-1} + log2(2x)] dx.

We can split into two integrals:

Integral A: ∫2^{x-1} dx from 1 to 2 =1/ln2.

Integral B: ∫log2(2x) dx from 1 to 2 =3 -1/ln2.

Adding A and B: 1/ln2 +3 -1/ln2 =3. So the exact answer is 3. That's surprising, but maybe correct.

Let me check with a numerical approximation. Let's compute the integral numerically. Let's compute the integral from 1 to 2 of 2^{x-1} + log2(2x) dx.

First, 2^{x-1} can be written as (1/2)2^x. So the integral of 2^{x-1} is (1/2) * (2^x / ln2) evaluated from 1 to 2. Which is (1/(2 ln2))(2^2 -2^1) = (1/(2 ln2))(4 -2)= (2)/(2 ln2)=1/ln2. Which matches.

For the log part, log2(2x) =1 + log2 x. The integral from 1 to 2 of 1 dx is 1. The integral of log2 x from 1 to 2 is (x log2 x - x/ln2) evaluated from 1 to 2. At 2: 2*1 -2/ln2. At 1: 0 -1/ln2. So difference is (2 -2/ln2) - (-1/ln2) =2 -1/ln2. So total log part is 1 +2 -1/ln2=3 -1/ln2. Then adding the first part 1/ln2 gives 3. So exact answer is 3. So numerically, 3 is exact. Therefore, the numerical approximation is 3.0000000000. But wait, is that possible?

Wait, but maybe I made a mistake in the integration. Let me check with a numerical example. Let's compute the integral numerically. For example, approximate the integral using a simple method like the trapezoidal rule with a few intervals.

Let's split the interval from 1 to 2 into two intervals: x=1, 1.5, 2.

Compute the function at these points:

At x=1: 2^{0} + log2(2*1) =1 + log2(2)=1+1=2.

At x=1.5: 2^{0.5} + log2(3). 2^0.5≈1.4142, log2(3)≈1.58496. So total≈1.4142 +1.58496≈3.0.

At x=2: 2^{1} + log2(4)=2 +2=4.

Using trapezoidal rule: the area is (0.5/2)[f(1) + 2f(1.5) + f(2)] = (0.25)[2 + 2*3.0 +4] =0.25*(2+6+4)=0.25*12=3. So even with two intervals, the trapezoidal rule gives exactly 3. That's interesting. So the exact answer is indeed 3. So the numerical approximation is exactly 3.0000000000.

But wait, that's possible? Because the function might be such that the integral is exactly 3. Let me check with another method. For example, Simpson's rule. For two intervals (n=2), Simpson's rule requires even number of intervals, but with n=2, which is even. Simpson's rule formula is (h/3)[f(a) +4f(a+h) +f(b)] where h=(b-a)/2. Here, h=0.5. So:

(0.5/3)[2 +4*3.0 +4] = (0.5/3)(2 +12 +4)= (0.5/3)(18)=0.5*6=3. Again, gives 3. So Simpson's rule also gives exactly 3. So that's a good sign that the exact answer is 3.

Therefore, the exact answer is 3, and the numerical approximation is 3.0000000000. So the final answer is {"answer": "3", "numerical_answer": "3.0000000000"}.
</think>

{"answer": "3", "numerical_answer": "3.0000000000"}