To compute the definite integral \(\int_{-4}^4 \lvert x^3 - x \rvert \, dx\), we follow these steps:

### Step 1: Identify the points where the integrand changes sign
The expression inside the absolute value is \(x^3 - x = x(x^2 - 1) = x(x - 1)(x + 1)\). The roots are \(x = -1\), \(x = 0\), and \(x = 1\). These points divide the interval \([-4, 4]\) into subintervals where the sign of \(x^3 - x\) is consistent. We determine the sign of \(x^3 - x\) in each subinterval:

- \((-4, -1)\): Test \(x = -2\): \((-2)^3 - (-2) = -8 + 2 = -6 < 0\) → \(\lvert x^3 - x \rvert = -x^3 + x\)
- \((-1, 0)\): Test \(x = -0.5\): \((-0.5)^3 - (-0.5) = -0.125 + 0.5 = 0.375 > 0\) → \(\lvert x^3 - x \rvert = x^3 - x\)
- \((0, 1)\): Test \(x = 0.5\): \((0.5)^3 - 0.5 = 0.125 - 0.5 = -0.375 < 0\) → \(\lvert x^3 - x \rvert = -x^3 + x\)
- \((1, 4)\): Test \(x = 2\): \(2^3 - 2 = 8 - 2 = 6 > 0\) → \(\lvert x^3 - x \rvert = x^3 - x\)

### Step 2: Split the integral into subintervals
Using the above analysis, we split the integral as follows:
\[
\int_{-4}^4 \lvert x^3 - x \rvert \, dx = \int_{-4}^{-1} (-x^3 + x) \, dx + \int_{-1}^0 (x^3 - x) \, dx + \int_{0}^1 (-x^3 + x) \, dx + \int_{1}^4 (x^3 - x) \, dx
\]

### Step 3: Compute each integral separately
1. \(\int_{-4}^{-1} (-x^3 + x) \, dx\):
\[
= -\left[ \frac{x^4}{4} \right]_{-4}^{-1} + \left[ \frac{x^2}{2} \right]_{-4}^{-1} = -\left( \frac{1}{4} - \frac{256}{4} \right) + \left( \frac{1}{2} - \frac{16}{2} \right) = \frac{255}{4} - \frac{15}{2} = \frac{255}{4} - \frac{30}{4} = \frac{225}{4}
\]

2. \(\int_{-1}^0 (x^3 - x) \, dx\):
\[
= \left[ \frac{x^4}{4} \right]_{-1}^0 - \left[ \frac{x^2}{2} \right]_{-1}^0 = \left( 0 - \frac{1}{4} \right) - \left( 0 - \frac{1}{2} \right) = -\frac{1}{4} + \frac{1}{2} = \frac{1}{4}
\]

3. \(\int_{0}^1 (-x^3 + x) \, dx\):
\[
= -\left[ \frac{x^4}{4} \right]_{0}^1 + \left[ \frac{x^2}{2} \right]_{0}^1 = -\left( \frac{1}{4} - 0 \right) + \left( \frac{1}{2} - 0 \right) = -\frac{1}{4} + \frac{1}{2} = \frac{1}{4}
\]

4. \(\int_{1}^4 (x^3 - x) \, dx\):
\[
= \left[ \frac{x^4}{4} \right]_{1}^4 - \left[ \frac{x^2}{2} \right]_{1}^4 = \left( \frac{256}{4} - \frac{1}{4} \right) - \left( \frac{16}{2} - \frac{1}{2} \right) = \frac{255}{4} - \frac{15}{2} = \frac{255}{4} - \frac{30}{4} = \frac{225}{4}
\]

### Step 4: Sum the results
\[
\frac{225}{4} + \frac{1}{4} + \frac{1}{4} + \frac{225}{4} = \frac{225 + 1 + 1 + 225}{4} = \frac{452}{4} = 113
\]

### Step 5: Numerical approximation
The exact result is \(113\), so the numerical approximation is \(113.0000000000\).

### Final Answer
```json
{"answer": "113", "numerical_answer": "113.0000000000"}
```