To solve the definite integral 

\[
\int\limits_{0}^{2}\frac{x^{-1/2}(2-x)^{-1/2}}{\sqrt{1+1 \times x(2-x)}}T_{3}\left(\sqrt{1+1 \times x(2-x)}\right)dx,
\]

where \( T_3 \) is the Chebyshev polynomial of the first kind of degree 3, we proceed with the following steps:

### Step 1: Simplify the Integrand

First, observe the expression inside the square root:

\[
1 + x(2 - x) = 1 + 2x - x^2 = 2 - (x - 1)^2.
\]

Letâ€™s make a substitution to simplify the integral. Let:

\[
u = \sqrt{1 + x(2 - x)} = \sqrt{2 - (x - 1)^2}.
\]

Then, the derivative of \( u \) with respect to \( x \) is:

\[
\frac{du}{dx} = \frac{-(x - 1)}{\sqrt{2 - (x - 1)^2}} = \frac{-(x - 1)}{u}.
\]

However, this substitution does not seem immediately helpful. Instead, consider the substitution:

\[
x = 1 + \sin\theta, \quad dx = \cos\theta \, d\theta.
\]

The limits of integration change as follows:
- When \( x = 0 \), \( \theta = -\pi/2 \).
- When \( x = 2 \), \( \theta = \pi/2 \).

Now, express the integrand in terms of \( \theta \):

\[
x = 1 + \sin\theta, \quad 2 - x = 1 - \sin\theta.
\]

The expression inside the square root becomes:

\[
1 + x(2 - x) = 1 + (1 + \sin\theta)(1 - \sin\theta) = 1 + 1 - \sin^2\theta = 2 - \sin^2\theta = 1 + \cos^2\theta.
\]

Thus,

\[
u = \sqrt{1 + \cos^2\theta}.
\]

The Chebyshev polynomial \( T_3(u) \) is:

\[
T_3(u) = 4u^3 - 3u.
\]

Now, the integrand becomes:

\[
\frac{x^{-1/2}(2 - x)^{-1/2}}{\sqrt{1 + x(2 - x)}} T_3(u) = \frac{(1 + \sin\theta)^{-1/2}(1 - \sin\theta)^{-1/2}}{\sqrt{1 + \cos^2\theta}} (4u^3 - 3u).
\]

Notice that:

\[
(1 + \sin\theta)^{-1/2}(1 - \sin\theta)^{-1/2} = (1 - \sin^2\theta)^{-1/2} = (\cos^2\theta)^{-1/2} = \frac{1}{|\cos\theta|}.
\]

Since \( \theta \in [-\pi/2, \pi/2] \), \( \cos\theta \geq 0 \), so \( |\cos\theta| = \cos\theta \). Thus, the integrand simplifies to:

\[
\frac{1}{\cos\theta} \cdot \frac{1}{\sqrt{1 + \cos^2\theta}} \cdot (4u^3 - 3u).
\]

Substituting \( u = \sqrt{1 + \cos^2\theta} \), we have:

\[
4u^3 - 3u = 4(1 + \cos^2\theta)^{3/2} - 3(1 + \cos^2\theta)^{1/2}.
\]

Thus, the integral becomes:

\[
\int_{-\pi/2}^{\pi/2} \frac{1}{\cos\theta} \cdot \frac{1}{\sqrt{1 + \cos^2\theta}} \cdot \left[4(1 + \cos^2\theta)^{3/2} - 3(1 + \cos^2\theta)^{1/2}\right] \cos\theta \, d\theta.
\]

The \( \cos\theta \) terms cancel out:

\[
\int_{-\pi/2}^{\pi/2} \frac{4(1 + \cos^2\theta)^{3/2} - 3(1 + \cos^2\theta)^{1/2}}{\sqrt{1 + \cos^2\theta}} \, d\theta.
\]

Simplify the integrand:

\[
\int_{-\pi/2}^{\pi/2} \left[4(1 + \cos^2\theta) - 3\right] \, d\theta = \int_{-\pi/2}^{\pi/2} (4 + 4\cos^2\theta - 3) \, d\theta = \int_{-\pi/2}^{\pi/2} (1 + 4\cos^2\theta) \, d\theta.
\]

Now, compute the integral:

\[
\int_{-\pi/2}^{\pi/2} (1 + 4\cos^2\theta) \, d\theta.
\]

Using the identity \( \cos^2\theta = \frac{1 + \cos 2\theta}{2} \):

\[
1 + 4\cos^2\theta = 1 + 2(1 + \cos 2\theta) = 3 + 2\cos 2\theta.
\]

Thus, the integral becomes:

\[
\int_{-\pi/2}^{\pi/2} (3 + 2\cos 2\theta) \, d\theta = 3\pi + 2 \cdot \frac{\sin 2\theta}{2} \Big|_{-\pi/2}^{\pi/2} = 3\pi + \sin 2\theta \Big|_{-\pi/2}^{\pi/2}.
\]

Evaluating the sine term:

\[
\sin 2\theta \Big|_{-\pi/2}^{\pi/2} = \sin \pi - \sin (-\pi) = 0 - 0 = 0.
\]

Therefore, the exact value of the integral is:

\[
3\pi.
\]

### Step 2: Numerical Approximation

The numerical approximation of \( 3\pi \) to 10 decimal places is:

\[
3\pi \approx 9.4247779608.
\]

### Final Answer

```json
{"answer": "3\\pi", "numerical_answer": "9.4247779608"}
```