To solve the definite integral 

\[
\int\limits_{0}^{2}\frac{x^{-1/2}(2-x)^{-1/2}}{\sqrt{1+1 \times x(2-x)}}T_{3}\left(\sqrt{1+1 \times x(2-x)}\right)dx,
\]

where \( T_3 \) is the Chebyshev polynomial of the first kind of degree 3, we proceed with the following steps:

### Step 1: Simplify the Integrand

First, observe the expression inside the square root:

\[
1 + x(2 - x) = 1 + 2x - x^2 = 2 - (x^2 - 2x + 1) = 2 - (x - 1)^2.
\]

Let us make a substitution to simplify the integral. Let:

\[
u = \sqrt{1 + x(2 - x)} = \sqrt{2 - (x - 1)^2}.
\]

Then, the derivative of \( u \) with respect to \( x \) is:

\[
\frac{du}{dx} = \frac{-2(x - 1)}{2\sqrt{2 - (x - 1)^2}} = \frac{-(x - 1)}{u}.
\]

However, this substitution does not seem immediately helpful. Instead, consider the substitution:

\[
x = 1 + \sin\theta, \quad dx = \cos\theta \, d\theta.
\]

The limits of integration change as follows:
- When \( x = 0 \), \( \theta = -\pi/2 \).
- When \( x = 2 \), \( \theta = \pi/2 \).

Now, express the integrand in terms of \( \theta \):

\[
x^{-1/2} = (1 + \sin\theta)^{-1/2}, \quad (2 - x)^{-1/2} = (1 - \sin\theta)^{-1/2},
\]

\[
1 + x(2 - x) = 2 - (x - 1)^2 = 2 - \sin^2\theta = 1 + \cos^2\theta,
\]

\[
u = \sqrt{1 + \cos^2\theta}, \quad T_3(u) = T_3\left(\sqrt{1 + \cos^2\theta}\right).
\]

The Chebyshev polynomial \( T_3 \) is given by:

\[
T_3(u) = 4u^3 - 3u.
\]

Thus, the integrand becomes:

\[
\frac{(1 + \sin\theta)^{-1/2}(1 - \sin\theta)^{-1/2}}{\sqrt{1 + \cos^2\theta}} \left(4(1 + \cos^2\theta)^{3/2} - 3\sqrt{1 + \cos^2\theta}\right) \cos\theta.
\]

Simplify the product:

\[
(1 + \sin\theta)^{-1/2}(1 - \sin\theta)^{-1/2} = (1 - \sin^2\theta)^{-1/2} = (\cos^2\theta)^{-1/2} = \frac{1}{|\cos\theta|}.
\]

Since \( \theta \in [-\pi/2, \pi/2] \), \( \cos\theta \geq 0 \), so \( |\cos\theta| = \cos\theta \). Thus, the integrand simplifies to:

\[
\frac{1}{\cos\theta} \cdot \frac{1}{\sqrt{1 + \cos^2\theta}} \left(4(1 + \cos^2\theta)^{3/2} - 3\sqrt{1 + \cos^2\theta}\right) \cos\theta
= \frac{4(1 + \cos^2\theta)^{3/2} - 3\sqrt{1 + \cos^2\theta}}{\sqrt{1 + \cos^2\theta}}
= 4(1 + \cos^2\theta) - 3 = 1 + 4\cos^2\theta.
\]

Now, the integral becomes:

\[
\int_{-\pi/2}^{\pi/2} (1 + 4\cos^2\theta) \, d\theta.
\]

### Step 2: Evaluate the Simplified Integral

Compute the integral:

\[
\int_{-\pi/2}^{\pi/2} (1 + 4\cos^2\theta) \, d\theta = \int_{-\pi/2}^{\pi/2} 1 \, d\theta + 4 \int_{-\pi/2}^{\pi/2} \cos^2\theta \, d\theta.
\]

The first integral is straightforward:

\[
\int_{-\pi/2}^{\pi/2} 1 \, d\theta = \pi.
\]

For the second integral, use the identity \( \cos^2\theta = \frac{1 + \cos 2\theta}{2} \):

\[
\int_{-\pi/2}^{\pi/2} \cos^2\theta \, d\theta = \int_{-\pi/2}^{\pi/2} \frac{1 + \cos 2\theta}{2} \, d\theta = \frac{1}{2} \left[ \theta + \frac{\sin 2\theta}{2} \right]_{-\pi/2}^{\pi/2} = \frac{\pi}{2}.
\]

Thus, the integral evaluates to:

\[
\pi + 4 \cdot \frac{\pi}{2} = \pi + 2\pi = 3\pi.
\]

### Step 3: Numerical Approximation

The exact answer is \( 3\pi \). A numerical approximation to 10 decimal places is:

\[
3\pi \approx 9.4247779608.
\]

### Final Answer

```json
{"answer": "3\\pi", "numerical_answer": "9.4247779608"}
```