<think>
Okay, let's tackle this integral ∫₀² H₃(√(x(2−x))) dx. Hmm, H₃ is the third Hermite polynomial. First, I need to recall what H₃ looks like. The Hermite polynomials are given by Hₙ(x) = (-1)ⁿ e^{x²} dⁿ/dxⁿ e^{-x²}. Let me remember the explicit form for n=3.

Wait, maybe there's a simpler way. The first few Hermite polynomials are known. Let me list them out. H₀(x) = 1, H₁(x) = 2x, H₂(x) = 4x² − 2, H₃(x) = 8x³ − 12x. Right, so H₃(y) = 8y³ − 12y. So substituting y = √(x(2−x)), the integrand becomes 8[√(x(2−x))]³ − 12√(x(2−x)}.

So the integral becomes ∫₀² [8(x(2−x))^(3/2) − 12(x(2−x))^(1/2)] dx. Let's factor out the constants: 8 ∫₀² [x(2−x)]^(3/2) dx − 12 ∫₀² [x(2−x)]^(1/2) dx.

Now, these integrals look like they might be related to Beta functions or Gamma functions. The integral of [x(2−x)]^k dx from 0 to 2. Let me make a substitution to simplify. Let’s set t = x − 1, which shifts the interval. Then x = t + 1, dx = dt, and when x=0, t=-1; x=2, t=1. But maybe a better substitution is to let u = x/2, so that the limits go from 0 to 1. Wait, perhaps a substitution. Let me think.

Alternatively, note that x(2−x) = 2x − x² = 1 − (x−1)². So completing the square, we have x(2−x) = 1 − (x−1)². So the integrand becomes [1 − (x−1)²]^{k} and [1 − (x−1)²]^{3/2} and [1 − (x−1)²]^{1/2}. That suggests a substitution of t = x−1, so the integral becomes from t=-1 to t=1 of [1 − t²]^{k} dt. That's symmetric, and the integral of [1−t²]^k from -1 to 1 is a standard Beta function integral. Specifically, ∫_{-1}^1 (1−t²)^k dt = 2 ∫₀¹ (1−t²)^k dt. Let me confirm that substitution. Let t = x−1, so when x=0, t=-1; x=2, t=1. Then dx = dt. So the integral becomes ∫_{-1}^1 [1−t²]^{k} dt. Which is 2 ∫₀¹ [1−t²]^{k} dt. Let’s set u = t², but maybe a better substitution is to use the Beta function. The integral ∫₀¹ t^{m} (1−t²)^n dt can be expressed in terms of Beta functions. Let me recall that ∫₀¹ t^{c-1} (1−t)^{d-1} dt = B(c, d) = Γ(c)Γ(d)/Γ(c+d). But here we have (1−t²)^k. Let’s set u = t², so t = sqrt(u), dt = (1/(2√u)) du. Then the integral becomes ∫₀¹ (1−u)^k * (1/(2√u)) du = (1/2) ∫₀¹ u^{-1/2} (1−u)^k du = (1/2) B(1/2, k+1) = (1/2) Γ(1/2)Γ(k+1)/Γ(k + 3/2). Since Γ(1/2) = √π, and Γ(k+1) = k! for integer k. So for the first integral, where k = 3/2, and the second integral where k = 1/2. Wait, but in our case, the exponent is [1−t²]^{k} where k is 3/2 and 1/2. Wait, no. Let me check. The original integral after substitution is ∫₀² [x(2−x)]^{n} dx = ∫_{-1}^1 [1−t²]^{n} dt = 2 ∫₀¹ [1−t²]^{n} dt. So for the first term, n=3/2, and the second term, n=1/2. So let's compute these two integrals.

First integral: 8 * 2 ∫₀¹ [1−t²]^{3/2} dt. Second integral: -12 * 2 ∫₀¹ [1−t²]^{1/2} dt. So total integral is 16 ∫₀¹ [1−t²]^{3/2} dt − 24 ∫₀¹ [1−t²]^{1/2} dt.

Now, compute each integral using the Beta function. For the first integral, ∫₀¹ [1−t²]^{3/2} dt. Let’s set u = t², so t = sqrt(u), dt = (1/(2√u)) du. Then the integral becomes ∫₀¹ (1−u)^{3/2} * (1/(2√u)) du = (1/2) ∫₀¹ u^{-1/2} (1−u)^{3/2} du. This is (1/2) B(1/2, 5/2) = (1/2) [Γ(1/2)Γ(5/2)/Γ(3)]. Since Γ(1/2) = √π, Γ(5/2) = (3/2)(1/2)√π = (3/4)√π, and Γ(3) = 2! = 2. So (1/2) [√π * (3/4)√π] / 2 = (1/2) * (3/4 π ) / 2 = (3/16) π. Wait, let me compute step by step:

Γ(1/2) = √π

Γ(5/2) = (3/2) Γ(3/2) = (3/2)(1/2)Γ(1/2) = (3/4)√π

Γ(3) = 2! = 2

So B(1/2, 5/2) = Γ(1/2)Γ(5/2)/Γ(3) = (√π)(3/4 √π) / 2 = (3/4 π) / 2 = 3π/8

Then (1/2) * B(1/2,5/2) = (1/2)(3π/8) = 3π/16

So the first integral ∫₀¹ [1−t²]^{3/2} dt = 3π/16

Similarly, the second integral ∫₀¹ [1−t²]^{1/2} dt. Using the same substitution:

∫₀¹ [1−t²]^{1/2} dt = (1/2) B(1/2, 3/2) = (1/2) [Γ(1/2)Γ(3/2)/Γ(2)]

Γ(3/2) = (1/2)Γ(1/2) = (1/2)√π

Γ(2) = 1! = 1

So B(1/2, 3/2) = (√π)(1/2 √π)/1 = (π/2)

Thus, (1/2) * (π/2) = π/4

Therefore, the second integral is π/4

Putting it all together:

The original integral is 16*(3π/16) - 24*(π/4) = 3π - 6π = -3π

Wait, that's interesting. Let me check the coefficients again.

Original integral after substitution:

8 * 2 ∫₀¹ [1−t²]^{3/2} dt − 12 * 2 ∫₀¹ [1−t²]^{1/2} dt

So 8*2 = 16, and 12*2=24. Then 16*(3π/16) = 3π, and 24*(π/4) = 6π. So 3π -6π = -3π. So the integral is -3π. But wait, integrating a real function over a real interval, and the integrand is H₃(√(x(2−x))). Let me check if H₃(y) =8y³−12y. So substituting y=√(x(2−x)), which is real and non-negative between 0 and 2. Then H₃(y) =8y³−12y. So the integrand is 8y³−12y. Let's check if the integral is negative. Let's see, when x is between 0 and 2, y=√(x(2−x)) is symmetric around x=1. The function y is a semicircle-like curve from 0 to 2, peaking at x=1 with y=1. So y ranges from 0 to 1. Then 8y³−12y = y(8y²−12). For y in [0,1], 8y²−12 is negative (since 8*1−12=−4). So the integrand is negative over the entire interval except at y=0 where it's zero. So the integral being negative makes sense. So -3π is plausible.

But let me verify the steps again. Let's recheck the substitution. The integral from 0 to 2 of H₃(√(x(2−x))) dx becomes 8 ∫ [x(2−x)]^{3/2} dx −12 ∫ [x(2−x)]^{1/2} dx. Then substitution t = x−1, leading to integrating [1−t²]^{3/2} and [1−t²]^{1/2} over t from -1 to 1, which is twice the integral from 0 to1. Then using Beta functions, which gave us 3π/16 and π/4. Then multiplying by 16 and 24 respectively. 16*(3π/16) is 3π, 24*(π/4) is 6π. So 3π−6π=−3π. So the exact answer is −3π. 

But wait, let me check if there's a miscalculation in the Beta function steps. For the first integral, [1−t²]^{3/2}:

The substitution gives (1/2) B(1/2, 5/2). B(a,b) = Γ(a)Γ(b)/Γ(a+b). So Γ(1/2)Γ(5/2)/Γ(3). Γ(5/2) is (3/2)(1/2)Γ(1/2) = (3/4)√π. So Γ(1/2)*Γ(5/2) = √π*(3/4 √π) = 3/4 π. Then Γ(3) is 2. So B(1/2,5/2) = (3/4 π)/2 = 3π/8. Then (1/2)*B(1/2,5/2) = 3π/16. Correct. Then 16*(3π/16) =3π. 

For the second integral, [1−t²]^{1/2}:

(1/2) B(1/2, 3/2). Γ(1/2)Γ(3/2) = √π*(1/2 √π) = (1/2)π. Γ(2) =1! =1. So B(1/2,3/2) = (1/2 π)/1 = π/2. Then (1/2)*π/2 = π/4. Then 24*(π/4) =6π. So 3π−6π=−3π. So the exact answer is −3π. 

Numerically, π is approximately 3.1415926536, so −3π ≈−9.4247779608. Let me check with a numerical approximation. Let's compute the integral numerically to confirm. Let's take x from 0 to 2, compute H3(sqrt(x(2−x))) dx. H3(y)=8y³−12y. So the integrand is 8*(x(2−x))^(3/2) −12*(x(2−x))^(1/2). Let's compute this integral numerically. Since the exact answer is −3π ≈−9.4247779608. Let's see if that's the case. Alternatively, maybe use substitution. Let me try to compute the integral. Let's split into two parts: 8*I3 −12*I1, where I3=∫₀² [x(2−x)]^{3/2} dx and I1=∫₀² [x(2−x)]^{1/2} dx. We already found analytically that I3=3π/8 and I1=π/2. So 8*(3π/8) −12*(π/2) =3π−6π=−3π. So yes, that's correct. Therefore, the exact answer is −3π, and the numerical approximation is approximately −9.4247779608. Rounded to 10 decimal places, that's -9.4247779608. But let me check with a calculator. π is approximately 3.141592653589793. So 3π is 9.42477796076938, so -3π is -9.42477796076938. Rounded to 10 decimal places, that's -9.4247779608. So the final answer should be {"answer": "-3\\pi", "numerical_answer": "-9.4247779608"}.
</think>

{"answer": "-3\\pi", "numerical_answer": "-9.4247779608"}