To solve the definite integral \(\int\limits_{0}^{2} x \arctan(\sqrt{x(2-x)}) \, dx\), we will follow the steps outlined:

### Step 1: Analytical Solution

First, let's make a substitution to simplify the integrand. Let \( t = \sqrt{x(2-x)} \). Then, we need to express \( x \) and \( dx \) in terms of \( t \).

From \( t = \sqrt{x(2-x)} \), we have:
\[ t^2 = x(2 - x) \]
\[ t^2 = 2x - x^2 \]
\[ x^2 - 2x + t^2 = 0 \]

Solving this quadratic equation for \( x \):
\[ x = \frac{2 \pm \sqrt{4 - 4t^2}}{2} \]
\[ x = 1 \pm \sqrt{1 - t^2} \]

Since \( x \) ranges from 0 to 2, we choose the appropriate branch:
\[ x = 1 + \sqrt{1 - t^2} \]

Next, we need \( dx \):
\[ dx = \frac{d}{dt} \left(1 + \sqrt{1 - t^2}\right) dt \]
\[ dx = \frac{-t}{\sqrt{1 - t^2}} dt \]

Now, substitute \( x \) and \( dx \) back into the integral:
\[ \int_{0}^{2} x \arctan(\sqrt{x(2-x)}) \, dx = \int_{0}^{1} (1 + \sqrt{1 - t^2}) \arctan(t) \cdot \frac{-t}{\sqrt{1 - t^2}} \, dt \]

Simplify the integrand:
\[ \int_{0}^{1} (1 + \sqrt{1 - t^2}) \arctan(t) \cdot \frac{-t}{\sqrt{1 - t^2}} \, dt = -\int_{0}^{1} \frac{t \arctan(t)}{\sqrt{1 - t^2}} \, dt - \int_{0}^{1} t \arctan(t) \, dt \]

Let's handle these integrals separately.

#### Integral 1: \(\int_{0}^{1} \frac{t \arctan(t)}{\sqrt{1 - t^2}} \, dt\)

Using integration by parts, let:
\[ u = \arctan(t) \quad \Rightarrow \quad du = \frac{1}{1 + t^2} dt \]
\[ dv = \frac{t}{\sqrt{1 - t^2}} dt \quad \Rightarrow \quad v = -\sqrt{1 - t^2} \]

Then:
\[ \int u \, dv = uv - \int v \, du \]
\[ \int_{0}^{1} \frac{t \arctan(t)}{\sqrt{1 - t^2}} \, dt = -\arctan(t) \sqrt{1 - t^2} \Big|_{0}^{1} + \int_{0}^{1} \frac{\sqrt{1 - t^2}}{1 + t^2} \, dt \]

Evaluating the boundary term:
\[ -\arctan(1) \sqrt{1 - 1^2} + \arctan(0) \sqrt{1 - 0^2} = 0 \]

So we are left with:
\[ \int_{0}^{1} \frac{\sqrt{1 - t^2}}{1 + t^2} \, dt \]

This integral is known and evaluates to:
\[ \int_{0}^{1} \frac{\sqrt{1 - t^2}}{1 + t^2} \, dt = \frac{\pi}{4} \]

#### Integral 2: \(\int_{0}^{1} t \arctan(t) \, dt\)

Using integration by parts again, let:
\[ u = \arctan(t) \quad \Rightarrow \quad du = \frac{1}{1 + t^2} dt \]
\[ dv = t \, dt \quad \Rightarrow \quad v = \frac{t^2}{2} \]

Then:
\[ \int u \, dv = uv - \int v \, du \]
\[ \int_{0}^{1} t \arctan(t) \, dt = \frac{t^2}{2} \arctan(t) \Big|_{0}^{1} - \int_{0}^{1} \frac{t^2}{2(1 + t^2)} \, dt \]

Evaluating the boundary term:
\[ \frac{1^2}{2} \arctan(1) - \frac{0^2}{2} \arctan(0) = \frac{\pi}{8} \]

So we are left with:
\[ \int_{0}^{1} \frac{t^2}{2(1 + t^2)} \, dt = \frac{1}{2} \int_{0}^{1} \left(1 - \frac{1}{1 + t^2}\right) dt \]
\[ = \frac{1}{2} \left[ t - \arctan(t) \right]_{0}^{1} \]
\[ = \frac{1}{2} \left(1 - \frac{\pi}{4}\right) \]
\[ = \frac{1}{2} - \frac{\pi}{8} \]

Combining the results:
\[ \int_{0}^{1} t \arctan(t) \, dt = \frac{\pi}{8} - \left(\frac{1}{2} - \frac{\pi}{8}\right) = \frac{\pi}{4} - \frac{1}{2} \]

### Step 2: Combine the Results

Combining the results of the two integrals:
\[ -\left(\frac{\pi}{4}\right) - \left(\frac{\pi}{4} - \frac{1}{2}\right) = -\frac{\pi}{2} + \frac{1}{2} \]

### Step 3: Numerical Approximation

The exact answer is:
\[ \frac{1}{2} - \frac{\pi}{2} \]

Numerical approximation:
\[ \frac{1}{2} - \frac{\pi}{2} \approx 0.5 - 1.57079632679 \approx -1.07079632679 \]

### Step 4: JSON Format

```json
{"answer": "\\frac{1}{2} - \\frac{\\pi}{2}", "numerical_answer": "-1.0707963268"}
```