Let's solve the integral:
\[
I = \int_0^{2} x^{-1/2}\,(2-x)^{-1/2}\,(1+0.5x)^{-2}\, T_2(\sqrt{1+0.5x})\, dx
\]
where \(T_2\) denotes the degree-2 Chebyshev polynomial of the first kind.

### Step 1. Expand the Chebyshev Polynomial

Recall:
\[
T_2(\xi) = 2\xi^2 - 1
\]
So,
\[
T_2(\sqrt{1+0.5x}) = 2(1+0.5x) - 1 = 2 + x - 1 = 1 + x
\]
Thus, the integrand becomes:
\[
x^{-1/2}\,(2-x)^{-1/2}\,(1+0.5x)^{-2}\,(1 + x)
\]

### Step 2. Split the Integral

Write as two terms:
\[
I = \int_0^{2} x^{-1/2} (2-x)^{-1/2} (1+0.5x)^{-2}\, dx
+ \int_0^{2} x^{1/2} (2-x)^{-1/2} (1+0.5x)^{-2}\, dx
\]
Let’s denote these as \(I_1\) and \(I_2\).

#### Substitute for simplicity

Let’s use \(x = 2\sin^2\theta\), for \(x \in [0,2] \implies \theta \in [0, \pi/2]\).

Compute the differentials and terms:
- \(x = 2\sin^2\theta\)
- \(dx = 4\sin\theta\cos\theta\, d\theta = 2\sin{2\theta}\, d\theta\)
- \(x^{-1/2} = (2\sin^2\theta)^{-1/2} = (2)^{-1/2}\sin^{-1}\theta\)
- \(x^{1/2} = (\sqrt{2})\sin\theta\)
- \(2-x = 2(1-\sin^2\theta) = 2\cos^2\theta\), so \((2-x)^{-1/2} = (2)^{-1/2}\cos^{-1}\theta\)
- \(1+0.5x = 1+0.5\cdot2\sin^2\theta = 1+\sin^2\theta\)
- \((1+0.5x)^{-2} = (1+\sin^2\theta)^{-2}\)

Now,
\[
I_1 = \int_{x=0}^{2} x^{-1/2}\,(2-x)^{-1/2}\,(1+0.5x)^{-2}\, dx
= \int_{\theta=0}^{\pi/2} (2)^{-1/2}\sin^{-1}\theta \cdot (2)^{-1/2}\cos^{-1}\theta \cdot (1+\sin^2\theta)^{-2} \cdot 2\sin 2\theta\, d\theta
\]

\[
= \int_{0}^{\pi/2} (2)^{-1}\sin^{-1}\theta\cos^{-1}\theta (1+\sin^2\theta)^{-2} \cdot 2\sin 2\theta\, d\theta
\]

\[
= \int_{0}^{\pi/2} (2)^{-1} \cdot 2\, \sin 2\theta\, \sin^{-1}\theta\cos^{-1}\theta (1+\sin^2\theta)^{-2} d\theta
\]

Recall: \(\sin 2\theta = 2\sin\theta\cos\theta\), so

\[
= \int_{0}^{\pi/2} (2)^{-1} \cdot 2 \cdot 2\sin\theta\cos\theta\, \sin^{-1}\theta\cos^{-1}\theta\, (1+\sin^2\theta)^{-2} d\theta
\]

\[
= \int_{0}^{\pi/2} (2)^{-1} \cdot 4 \cdot \sin\theta\cos\theta\, \sin^{-1}\theta\cos^{-1}\theta\, (1+\sin^2\theta)^{-2} d\theta
\]

Note: \(\sin\theta\,\sin^{-1}\theta = 1\), \(\cos\theta\,\cos^{-1}\theta = 1\), so

\[
= \int_{0}^{\pi/2} 2 \cdot (1+\sin^2\theta)^{-2} d\theta
\]

So,
\[
I_1 = 2 \int_{0}^{\pi/2} (1+\sin^2\theta)^{-2} d\theta
\]

Similarly, work through \(I_2\):

\[
I_2 = \int_{x=0}^{2} x^{1/2} (2-x)^{-1/2} (1+0.5x)^{-2}\, dx
\]
\[
= \int_{0}^{\pi/2} (\sqrt{2}) \sin\theta \cdot (2)^{-1/2} \cos^{-1}\theta \cdot (1+\sin^2\theta)^{-2} \cdot 2\sin 2\theta\, d\theta
\]
\[
= \int_{0}^{\pi/2} (\sqrt{2})(2)^{-1/2} \sin\theta \cos^{-1}\theta\, (1+\sin^2\theta)^{-2} 2\sin 2\theta\, d\theta
\]
\[
(\sqrt{2})(2)^{-1/2} = 2^{1/2} \cdot 2^{-1/2} = 1
\]
Thus,
\[
I_2 = \int_{0}^{\pi/2} \sin\theta\cos^{-1}\theta (1+\sin^2\theta)^{-2} 2\sin 2\theta d\theta
\]
As above, \(\sin 2\theta = 2\sin\theta\cos\theta\):

\[
= \int_{0}^{\pi/2} 2\sin\theta\cos^{-1}\theta (1+\sin^2\theta)^{-2} 2\sin\theta\cos\theta\, d\theta
\]
\[
= \int_{0}^{\pi/2} 4 \sin^2\theta\, \cos^{0}\theta\, (1+\sin^2\theta)^{-2}\, d\theta
\]
\[
= 4 \int_{0}^{\pi/2} \sin^2\theta\, (1+\sin^2\theta)^{-2}\, d\theta
\]

### Step 3. Combine the Parts

\[
I = I_1 + I_2 = 2 \int_0^{\pi/2} (1+\sin^2\theta)^{-2}\, d\theta + 4 \int_0^{\pi/2} \frac{\sin^2\theta}{(1+\sin^2\theta)^2} d\theta
\]

Combine to a single integral:
\[
I = \int_0^{\pi/2} \frac{2 + 4\sin^2\theta}{(1+\sin^2\theta)^2} d\theta
= 2 \int_0^{\pi/2} \frac{1 + 2\sin^2\theta}{(1+\sin^2\theta)^2}\, d\theta
\]

### Step 4. Simplification

Let’s try to simplify \(\frac{1 + 2\sin^2\theta}{(1+\sin^2\theta)^2}\):

Let’s use substitution to split numerator:
\[
1 + 2\sin^2\theta = (1+\sin^2\theta) + \sin^2\theta
\]
So,
\[
\frac{1+2\sin^2\theta}{(1+\sin^2\theta)^2} = \frac{1+\sin^2\theta}{(1+\sin^2\theta)^2} + \frac{\sin^2\theta}{(1+\sin^2\theta)^2}
= \frac{1}{1+\sin^2\theta} + \frac{\sin^2\theta}{(1+\sin^2\theta)^2}
\]

Therefore,
\[
I = 2 \int_{0}^{\pi/2} \left[\frac{1}{1+\sin^2\theta} + \frac{\sin^2\theta}{(1+\sin^2\theta)^2}\right] d\theta
\]

Thus,
\[
I = 2 \int_{0}^{\pi/2} \frac{1}{1+\sin^2\theta} d\theta
+ 2 \int_{0}^{\pi/2} \frac{\sin^2\theta}{(1+\sin^2\theta)^2} d\theta
\]

Now denote:
\[
A = \int_0^{\pi/2} \frac{1}{1+\sin^2\theta} d\theta
\]
\[
B = \int_0^{\pi/2} \frac{\sin^2\theta}{(1+\sin^2\theta)^2} d\theta
\]

So \[
I = 2A + 2B \ .

\]

#### Compute \(B\):

But notice that:
\[
\frac{d}{d\theta}\left(-\frac{1}{1+\sin^2\theta}\right)
= -\frac{d}{d\theta}(1+\sin^2\theta)^{-1}
= (1+\sin^2\theta)^{-2} \cdot 2\sin\theta\cos\theta
= \frac{2\sin\theta\cos\theta}{(1+\sin^2\theta)^2}
\]
But the numerator here was \(\sin^2\theta\); let's try manipulating...

Alternatively, observe that:

\[
\frac{\sin^2\theta}{(1+\sin^2\theta)^2} = \frac{1}{1+\sin^2\theta} - \frac{1}{(1+\sin^2\theta)}
+ \frac{1}{(1+\sin^2\theta)} - \frac{1}{(1+\sin^2\theta)^2}
\]
But this does not seem to help much.

Alternatively, express \(B\) in terms of \(A\):

Let’s try integrating by parts:

Let’s try the substitution \(u = \tan\theta\):

For \( \theta \in [0, \pi/2) \), \( u \in [0,\infty) \).

\[
\sin\theta = \frac{u}{\sqrt{1+u^2}}
\]
\[
d\theta = \frac{1}{1+u^2} du
\]

\[
\sin^2\theta = \frac{u^2}{1+u^2}
\]
\[
1+\sin^2\theta = 1+\frac{u^2}{1+u^2} = \frac{1+u^2+u^2}{1+u^2} = \frac{1+2u^2}{1+u^2}
\]
\[
(1+\sin^2\theta)^{-1} = \frac{1+u^2}{1+2u^2}
\]
So,
\[
A = \int_0^{\pi/2} \frac{1}{1+\sin^2\theta} d\theta = \int_{u=0}^{\infty} \frac{1+u^2}{1+2u^2}\cdot \frac{1}{1+u^2} du = \int_0^\infty \frac{1}{1+2u^2}\, du
\]

Similarly,
\[
B = \int_0^{\pi/2} \frac{\sin^2\theta}{(1+\sin^2\theta)^2} d\theta
\]
\[
\sin^2\theta = \frac{u^2}{1+u^2}
\]
\[
(1+\sin^2\theta)^2 = \left(\frac{1+2u^2}{1+u^2}\right)^2 = \frac{(1+2u^2)^2}{(1+u^2)^2}
\]

Thus,
\[
\frac{\sin^2\theta}{(1+\sin^2\theta)^2} = \frac{u^2}{1+u^2} \cdot \frac{(1+u^2)^2}{(1+2u^2)^2} = \frac{u^2 (1+u^2)}{(1+2u^2)^2}
\]

So,
\[
B = \int_{0}^{\infty} \frac{u^2 (1+u^2)}{(1+2u^2)^2} \cdot \frac{du}{1+u^2}
= \int_{0}^{\infty} \frac{u^2}{(1+2u^2)^2}\, du
\]

Thus, after substitution,
\[
I = 2 \int_0^\infty \frac{1}{1+2u^2} du
+ 2 \int_0^\infty \frac{u^2}{(1+2u^2)^2} du
\]

### Step 5. Compute the Integrals

First:
\[
A = \int_0^{\infty} \frac{1}{1+2u^2} du = \frac{1}{\sqrt{2}} \int_0^{\infty} \frac{1}{1+v^2} dv
\]
where \(v = u\sqrt{2} \implies du = dv/\sqrt{2}\):

\[
A = \frac{1}{\sqrt{2}}\int_0^{\infty} \frac{1}{1+v^2} dv = \frac{1}{\sqrt{2}} \frac{\pi}{2}
= \frac{\pi}{2\sqrt{2}}
\]

Now:
\[
B = \int_0^{\infty} \frac{u^2}{(1+2u^2)^2} du
\]

Let’s use the substitution \(w = u^2\):
- When \(u=0, w=0\). \(u\to\infty \implies w\to\infty\).
- \(du = \frac{1}{2w^{1/2}}dw\)
- \(u^2 = w\)
So,
\[
B = \int_0^\infty \frac{w}{(1+2w)^2} \frac{dw}{2w^{1/2}}
= \frac{1}{2} \int_0^\infty \frac{w^{1/2}}{(1+2w)^2} dw
\]

Alternatively, use another substitution for simplicity.

Let’s perform partial fraction decomposition:
\[
\frac{u^2}{(1+2u^2)^2}
= \frac{1}{2} \left(\frac{1}{1+2u^2} - \frac{1}{(1+2u^2)^2}\right)
\]
**Check:**

\[
\frac{1}{2}\left(\frac{1}{1+2u^2} - \frac{1}{(1+2u^2)^2}\right)
= \frac{1}{2} \cdot \frac{(1+2u^2) - 1}{(1+2u^2)^2}
= \frac{2u^2}{2(1+2u^2)^2}
= \frac{u^2}{(1+2u^2)^2}
\]
This is correct.

So,
\[
B = \int_0^\infty \frac{u^2}{(1+2u^2)^2} du
= \frac{1}{2} \int_0^\infty \frac{1}{1+2u^2} du
- \frac{1}{2} \int_0^\infty \frac{1}{(1+2u^2)^2}\, du
\]

But the first term is \(A\) as above. Let’s compute the second integral:

Let’s let \(w = u \sqrt{2}\),
- \(u = w/\sqrt{2}\) so \(du = dw/\sqrt{2}\)
So,
\[
\int_0^\infty \frac{1}{(1+2u^2)^2} du = \int_0^\infty \frac{1}{(1 + w^2)^2} \frac{dw}{\sqrt{2}}
= \frac{1}{\sqrt{2}} \int_0^\infty \frac{1}{(1 + w^2)^2} dw
\]

Recall from tables:
\[
\int_0^\infty \frac{1}{(1 + w^2)^2} dw = \frac{\pi}{4}
\]

So,
\[
\int_0^\infty \frac{1}{(1+2u^2)^2} du = \frac{1}{\sqrt{2}} \cdot \frac{\pi}{4} = \frac{\pi}{4\sqrt{2}}
\]

Therefore,
\[
B = \frac{1}{2}A - \frac{1}{2} \cdot \frac{\pi}{4\sqrt{2}}
= \frac{1}{2}\left(\frac{\pi}{2\sqrt{2}}\right) - \frac{\pi}{8\sqrt{2}}
= \frac{\pi}{4\sqrt{2}} - \frac{\pi}{8\sqrt{2}} = \frac{\pi}{8\sqrt{2}}
\]

Now, use these in the formula for \(I\):

### Step 6. Final Combination

\[
I = 2A + 2B = 2\left(\frac{\pi}{2\sqrt{2}}\right) + 2\left(\frac{\pi}{8\sqrt{2}}\right)
= \frac{\pi}{\sqrt{2}} + \frac{\pi}{4\sqrt{2}}
= \frac{5\pi}{4\sqrt{2}}
\]

### Step 7. Numerical Evaluation

\[
I = \frac{5\pi}{4\sqrt{2}}
\]

Calculate numerically:
- \(\pi \approx 3.141592653589793\)
- \(\sqrt{2} \approx 1.4142135623730951\)

So,
\[
\frac{5\pi}{4\sqrt{2}} = \frac{5 \times 3.141592653589793}{4 \times 1.4142135623730951}
= \frac{15.707963267949465}{5.65685424949238}
\approx 2.778417889236835
\]

Rounded to ten decimal places: 2.7784178892

---

```json
{"answer": "\\frac{5\\pi}{4\\sqrt{2}}", "numerical_answer": "2.7784178892"}
```