

To solve the definite integral \(\int_0^1 (x-1)^2(x+1)^2(x^2+1)^2(x^4+1)^2 \, dx\), we start by simplifying the integrand using algebraic identities.

### Step 1: Simplify the integrand
First, observe that:
\[
(x-1)^2(x+1)^2 = \left[(x-1)(x+1)\right]^2 = (x^2 - 1)^2
\]
Next, multiply this result with \((x^2 + 1)^2\):
\[
(x^2 - 1)^2(x^2 + 1)^2 = \left[(x^2 - 1)(x^2 + 1)\right]^2 = (x^4 - 1)^2
\]
Finally, multiply by \((x^4 + 1)^2\):
\[
(x^4 - 1)^2(x^4 + 1)^2 = \left[(x^4 - 1)(x^4 + 1)\right]^2 = (x^8 - 1)^2
\]
Thus, the integrand simplifies to \((x^8 - 1)^2\).

### Step 2: Expand the simplified integrand
Expanding \((x^8 - 1)^2\) gives:
\[
(x^8 - 1)^2 = x^{16} - 2x^8 + 1
\]

### Step 3: Integrate term-by-term
The integral becomes:
\[
\int_0^1 (x^{16} - 2x^8 + 1) \, dx
\]
Integrate each term separately:
\[
\int x^{16} \, dx = \frac{x^{17}}{17}, \quad \int -2x^8 \, dx = -\frac{2x^9}{9}, \quad \int 1 \, dx = x
\]
Combining these results, the antiderivative is:
\[
\frac{x^{17}}{17} - \frac{2x^9}{9} + x
\]

### Step 4: Evaluate the definite integral
Evaluate the antiderivative at the bounds \(x=1\) and \(x=0\):
- At \(x=1\): \(\frac{1}{17} - \frac{2}{9} + 1\)
- At \(x=0\): \(0 - 0 + 0 = 0\)

Simplify the expression at \(x=1\):
\[
\frac{1}{17} - \frac{2}{9} + 1 = \frac{9}{153} - \frac{34}{153} + \frac{153}{153} = \frac{9 - 34 + 153}{153} = \frac{128}{153}
\]

### Step 5: Numerical approximation
The exact value is \(\frac{128}{153}\). To approximate this numerically:
\[
\frac{128}{153} \approx 0.8366013072
\]

{"answer": "\(\dfrac{128}{153}\)", "numerical_answer": "0.8366013072"}