<think>
Okay, let's tackle this integral step by step. The integral given is from 0 to 2 of x^(-1/2)(2 - x)^(-1/2)(1 + 0.5x)^(-2) T_{2×1}(√(1 + 0.5x)) dx. Hmm, first, I need to understand each part of this integrand. 

Starting with the terms x^(-1/2) and (2 - x)^(-1/2). These look like parts of a Beta function or maybe related to a substitution that can simplify the integral. The Beta function typically involves integrals of the form x^(a-1)(1 - x)^(b-1) from 0 to 1, so maybe a substitution can bring this into that form. 

Then there's the term (1 + 0.5x)^(-2). That's a bit more complicated. Also, the function T_{2×1}(√(1 + 0.5x)) is mentioned. Wait, T_{2×1}... I need to figure out what that notation means. Maybe it's a Chebyshev polynomial of the first kind, T_n(x), where n is 2×1? Wait, 2×1 is 2, so maybe it's T_2? But the argument is sqrt(1 + 0.5x). Let me confirm. Chebyshev polynomials of the first kind are denoted T_n(x), so T_2(x) would be 2x^2 - 1. So substituting sqrt(1 + 0.5x) into T_2 would give 2*(sqrt(1 + 0.5x))^2 - 1 = 2*(1 + 0.5x) - 1 = 2 + x - 1 = 1 + x. So T_{2×1} here is T_2, and when evaluated at sqrt(1 + 0.5x), it simplifies to 1 + x. That seems manageable.

So replacing T_{2×1}(sqrt(1 + 0.5x)) with 1 + x. Let me check that again. If T_n(x) is the Chebyshev polynomial of the first kind, then T_2(x) = 2x² - 1. So substituting sqrt(1 + 0.5x) into T_2 gives 2*(sqrt(1 + 0.5x))² - 1 = 2*(1 + 0.5x) -1 = 2 + x -1 = 1 + x. Yes, that's correct. So the integrand simplifies to x^(-1/2)(2 - x)^(-1/2)(1 + 0.5x)^(-2)(1 + x) dx from 0 to 2.

Now, let's write that out:

Integral from 0 to 2 of [x^{-1/2} (2 - x)^{-1/2} (1 + 0.5x)^{-2} (1 + x)] dx.

Hmm, maybe we can make a substitution to simplify the integral. Let's consider substitution variables. The limits are from 0 to 2, and the terms x and 2 - x suggest a substitution like t = x/2, which would map the interval [0,2] to [0,1]. Let's try that. Let t = x/2, so x = 2t, dx = 2dt. Then, when x=0, t=0; x=2, t=1. Substitute into the integral:

Integral from t=0 to t=1 of [(2t)^{-1/2} (2 - 2t)^{-1/2} (1 + 0.5*(2t))^{-2} (1 + 2t)] * 2 dt.

Simplify each term:

(2t)^{-1/2} = (2)^{-1/2} t^{-1/2}

(2 - 2t)^{-1/2} = (2(1 - t))^{-1/2} = (2)^{-1/2} (1 - t)^{-1/2}

(1 + 0.5*(2t)) = 1 + t, so (1 + t)^{-2}

(1 + 2t) remains as is.

Multiply all together along with the 2 from dx:

2 * [ (2^{-1/2} t^{-1/2}) * (2^{-1/2} (1 - t)^{-1/2}) * (1 + t)^{-2} * (1 + 2t) ] dt

Combine the constants: 2 * (2^{-1/2} * 2^{-1/2}) = 2 * (2^{-1}) = 2*(1/2) = 1.

So the integral simplifies to:

Integral from 0 to 1 of [ t^{-1/2} (1 - t)^{-1/2} (1 + t)^{-2} (1 + 2t) ] dt.

Hmm, that's better. Now, the integrand is t^{-1/2}(1 - t)^{-1/2} times (1 + t)^{-2}(1 + 2t). Let's see if we can simplify (1 + t)^{-2}(1 + 2t). Let's compute that term:

(1 + 2t)/(1 + t)^2. Let's see if this can be expressed as a derivative or something. Alternatively, perhaps split the fraction:

(1 + 2t)/(1 + t)^2 = [ (1 + t) + t ] / (1 + t)^2 = 1/(1 + t) + t/(1 + t)^2. But I'm not sure if that helps. Alternatively, maybe perform substitution. Let me check.

Alternatively, note that t^{-1/2}(1 - t)^{-1/2} is the Beta function integrand. The integral from 0 to 1 of t^{-1/2}(1 - t)^{-1/2} dt is B(1/2, 1/2) = π. But here we have an extra factor of (1 + 2t)/(1 + t)^2. So perhaps expanding this factor in terms that can be integrated with the Beta function.

Alternatively, consider substitution u = t/(1 + t). Let me try that. Let u = t/(1 + t), then t = u/(1 - u), dt = du/(1 - u)^2. When t=0, u=0; t=1, u=1/2. Hmm, not sure if that helps. Let's compute the integrand in terms of u:

t = u/(1 - u), 1 + t = 1 + u/(1 - u) = 1/(1 - u), 1 + 2t = 1 + 2u/(1 - u) = (1 - u + 2u)/(1 - u) = (1 + u)/(1 - u). Then:

(1 + 2t)/(1 + t)^2 = [ (1 + u)/(1 - u) ] / [1/(1 - u)]^2 = (1 + u)/(1 - u) * (1 - u)^2 = (1 + u)(1 - u) = 1 - u^2.

So the integrand becomes:

t^{-1/2}(1 - t)^{-1/2} * (1 + 2t)/(1 + t)^2 = [ (u/(1 - u))^{-1/2} (1 - u/(1 - u))^{-1/2} ] * (1 - u^2) * [du/(1 - u)^2]

Wait, let's compute each part:

t^{-1/2} = (u/(1 - u))^{-1/2} = ( (1 - u)/u )^{1/2 }

1 - t = 1 - u/(1 - u) = (1 - u - u)/ (1 - u) = (1 - 2u)/(1 - u). Wait, that can't be right. Wait, 1 - t = 1 - [u/(1 - u)] = [ (1 - u) - u ] / (1 - u) ) = (1 - 2u)/(1 - u). Hmm, but this seems complicated. Maybe this substitution isn't helpful. Let me check again.

Alternatively, perhaps expand (1 + 2t)/(1 + t)^2. Let's compute:

(1 + 2t)/(1 + t)^2 = A/(1 + t) + B/(1 + t)^2. Let's find A and B.

Multiply both sides by (1 + t)^2:

1 + 2t = A(1 + t) + B.

Set t = -1: Left side: 1 + 2*(-1) = -1. Right side: A(0) + B => B = -1.

Then, for other t, 1 + 2t = A(1 + t) -1. Rearranged: 1 + 2t +1 = A(1 + t) => 2 + 2t = A(1 + t) => A = 2.

So, (1 + 2t)/(1 + t)^2 = 2/(1 + t) - 1/(1 + t)^2.

Therefore, the integral becomes:

Integral from 0 to 1 of t^{-1/2}(1 - t)^{-1/2} [2/(1 + t) - 1/(1 + t)^2] dt.

So split into two integrals:

2 * Integral [ t^{-1/2}(1 - t)^{-1/2}/(1 + t) ] dt - Integral [ t^{-1/2}(1 - t)^{-1/2}/(1 + t)^2 ] dt.

Now, these integrals might be expressible in terms of Beta functions or hypergeometric functions. Let's recall that integrals of the form ∫ t^{c-1}(1 - t)^{d - c -1}/(1 + zt)^s dt from 0 to 1 relate to hypergeometric functions or Appell functions, but maybe there's a simpler approach here.

Alternatively, consider substitution u = t/(1 + t). Wait, let's try substitution for the first integral. Let u = t/(1 + t), so t = u/(1 - u), dt = du/(1 - u)^2. When t=0, u=0; t=1, u=1/2. Then, 1 + t = 1/(1 - u). Let's substitute into the first integral:

Integral [ t^{-1/2}(1 - t)^{-1/2}/(1 + t) ] dt from 0 to1 becomes:

Integral from u=0 to u=1/2 of [ (u/(1 - u))^{-1/2} (1 - u/(1 - u))^{-1/2} / (1/(1 - u)) ) ] * [ du/(1 - u)^2 ]

Simplify each term:

(u/(1 - u))^{-1/2} = ( (1 - u)/u )^{1/2 }

1 - t = 1 - u/(1 - u) = (1 - u - u)/(1 - u) = (1 - 2u)/(1 - u)

So (1 - t)^{-1/2} = ( (1 - 2u)/(1 - u) )^{-1/2} = (1 - u)^{1/2} (1 - 2u)^{-1/2}

Then, the denominator (1 + t) is 1/(1 - u), so dividing by that is multiplying by (1 - u).

Putting it all together:

[ (1 - u)/u )^{1/2 } * (1 - u)^{1/2} (1 - 2u)^{-1/2} ] * (1 - u) * [ du/(1 - u)^2 ]

Simplify exponents:

(1 - u)^{1/2} * (1 - u)^{1/2} = (1 - u)^1

Multiply by (1 - u): (1 - u)^2

Divide by (1 - u)^2: cancels out.

So remaining terms:

(1/u)^{1/2} * (1 - 2u)^{-1/2} * du

So the integral becomes:

Integral from u=0 to u=1/2 of u^{-1/2} (1 - 2u)^{-1/2} du.

Hmm, this seems more manageable. Let's make another substitution here. Let v = 2u, so u = v/2, du = dv/2. When u=0, v=0; u=1/2, v=1.

Then the integral becomes:

Integral from v=0 to v=1 of (v/2)^{-1/2} (1 - v)^{-1/2} * (dv/2)

Simplify:

(2^{1/2} v^{-1/2}) (1 - v)^{-1/2} * (1/2) dv

= 2^{1/2} * 1/2 * Integral v^{-1/2}(1 - v)^{-1/2} dv from 0 to1

= 2^{-1/2} * B(1/2, 1/2)

But B(1/2, 1/2) = π, so this integral is 2^{-1/2} * π? Wait, no. Wait, B(1/2,1/2) = Γ(1/2)^2 / Γ(1) = π / 1 = π. So the integral becomes 2^{-1/2} * π.

So the first integral (multiplied by 2) is 2 * [2^{-1/2} π] = 2^{1 - 1/2} π = 2^{1/2} π = sqrt(2) π.

Now, the second integral: Integral [ t^{-1/2}(1 - t)^{-1/2}/(1 + t)^2 ] dt from 0 to1.

This seems more complicated. Let's try the same substitution u = t/(1 + t). Then t = u/(1 - u), dt = du/(1 - u)^2, 1 + t = 1/(1 - u). So substituting into the integral:

Integral from u=0 to u=1/2 of [ (u/(1 - u))^{-1/2} (1 - u/(1 - u))^{-1/2} / (1/(1 - u))^2 ] * [ du/(1 - u)^2 ]

Simplify each term:

(u/(1 - u))^{-1/2} = ( (1 - u)/u )^{1/2 }

1 - t = 1 - u/(1 - u) = (1 - 2u)/(1 - u), so (1 - t)^{-1/2} = (1 - u)^{1/2} (1 - 2u)^{-1/2}

Denominator (1 + t)^2 = (1/(1 - u))^2, so dividing by that is multiplying by (1 - u)^2.

Putting it all together:

[ ( (1 - u)/u )^{1/2 } * (1 - u)^{1/2} (1 - 2u)^{-1/2} ] * (1 - u)^2 * [ du/(1 - u)^2 ]

Simplify exponents:

(1 - u)^{1/2} * (1 - u)^{1/2} = (1 - u)^1

Multiply by (1 - u)^2: (1 - u)^3

Divide by (1 - u)^2: (1 - u)^1

So remaining terms:

(1/u)^{1/2} (1 - 2u)^{-1/2} (1 - u) du

So the integral becomes:

Integral from u=0 to u=1/2 of u^{-1/2} (1 - 2u)^{-1/2} (1 - u) du.

Hmm, this is similar to the previous integral but with an extra (1 - u) term. Let's again substitute v = 2u, so u = v/2, du = dv/2. Then when u=0, v=0; u=1/2, v=1.

Substituting:

Integral from v=0 to v=1 of (v/2)^{-1/2} (1 - v)^{-1/2} (1 - v/2) * (dv/2)

Simplify:

(2)^{1/2} v^{-1/2} (1 - v)^{-1/2} (1 - v/2) * (1/2) dv

= 2^{1/2} * 1/2 * Integral v^{-1/2} (1 - v)^{-1/2} (1 - v/2) dv

= 2^{-1/2} [ Integral v^{-1/2} (1 - v)^{-1/2} dv - (1/2) Integral v^{1/2} (1 - v)^{-1/2} dv ] from 0 to1.

Wait, expanding (1 - v/2) as 1 - (v/2):

= 2^{-1/2} [ Integral v^{-1/2}(1 - v)^{-1/2} dv - (1/2) Integral v^{1/2}(1 - v)^{-1/2} dv ]

Compute each integral separately.

First integral: Integral v^{-1/2}(1 - v)^{-1/2} dv from 0 to1 is B(1/2, 1/2) = π.

Second integral: Integral v^{1/2}(1 - v)^{-1/2} dv from 0 to1 is B(3/2, 1/2) = Γ(3/2)Γ(1/2)/Γ(2) = ( (sqrt(π)/2) * sqrt(π) ) / 1! ) = (π/2) / 1 = π/2.

So substituting back:

= ^{-1/2} [ π - (1/2)(π/2) ] = 2^{-1/2} [ π - π/4 ] = 2^{-1/2} * (3π/4) = 3π/(4 * 2^{1/2}) = 3π/(4 sqrt(2)).

Therefore, the second integral is 3π/(4 sqrt(2)).

Putting it all together, the original integral is:

First part (2 * first integral) - second integral = sqrt(2) π - 3π/(4 sqrt(2)).

Let's compute this:

sqrt(2) π = (4 sqrt(2) π)/(4), so:

(4 sqrt(2) π - 3 π)/(4 sqrt(2)) = π (4 sqrt(2) - 3)/(4 sqrt(2)).

But let's rationalize the denominator:

Multiply numerator and denominator by sqrt(2):

π (4 sqrt(2) - 3) sqrt(2) / (4 * 2) = π (4*2 - 3 sqrt(2)) / 8 = π (8 - 3 sqrt(2)) /8.

Wait, wait, let's do that step again:

Original expression: [sqrt(2) π - 3π/(4 sqrt(2))] = π [ sqrt(2) - 3/(4 sqrt(2)) ]

Combine terms by getting a common denominator:

= π [ (sqrt(2) * 4 sqrt(2) - 3 ) / (4 sqrt(2)) ]

Compute numerator: sqrt(2)*4 sqrt(2) = 4*2 = 8, so numerator is 8 - 3 = 5? Wait, no:

Wait, sqrt(2) * 4 sqrt(2) = 4*(sqrt(2))^2 = 4*2=8. Then subtract 3: 8 -3 =5. So:

= π (5)/(4 sqrt(2)) = (5 π)/(4 sqrt(2)).

Rationalizing the denominator:

= (5 π)/(4 sqrt(2)) * sqrt(2)/sqrt(2) = (5 π sqrt(2))/8.

So the exact value is (5 sqrt(2) π)/8.

Now, let's compute the numerical approximation. Compute sqrt(2) ≈ 1.41421356237, π ≈ 3.141592653589793.

Multiply them: 1.41421356237 * 3.141592653589793 ≈ 4.442882908158179.

Then multiply by 5: 4.442882908158179 *5 ≈ 22.214414540790895.

Divide by 8: 22.214414540790895 /8 ≈ 2.7768018175988617.

Rounded to 10 decimal places: 2.7768018176.

Wait, but let me check the calculation again to be precise.

First, sqrt(2) ≈ 1.41421356237

π ≈ 3.141592653589793

Multiply sqrt(2) and π: 1.41421356237 * 3.141592653589793 ≈

Let me compute this step by step:

1.41421356237 * 3 = 4.24264068711

1.41421356237 * 0.141592653589793 ≈

Compute 1.41421356237 * 0.1 = 0.141421356237

1.41421356237 * 0.041592653589793 ≈

Approximate 0.04 *1.41421356237 = 0.05656854249

0.001592653589793 *1.41421356237 ≈ ~0.002252

So total for 0.041592653589793: ~0.05656854249 + 0.002252 ≈ 0.05882

So total 0.141592653589793 ≈ 0.141421356237 +0.05882 ≈ 0.200241356237

So total sqrt(2)*π ≈ 4.24264068711 +0.200241356237 ≈ 4.442882043347

Then multiply by 5: 4.442882043347 *5 = 22.214410216735

Divide by 8: 22.214410216735 /8 = 2.776801277091875

Rounded to 10 decimal places: 2.7768012771. Wait, but earlier I had 2.7768018176. There's a discrepancy here. Let me use a calculator.

Alternatively, use exact computation:

5 * sqrt(2) * π /8.

Compute sqrt(2) = 1.4142135623730950488016887242097

π = 3.1415926535897932384626433832795

Multiply sqrt(2) * π: 1.4142135623730950488016887242097 * 3.1415926535897932384626433832795 ≈

Let me compute this precisely:

1.4142135623730950488 * 3.14159265358979323846 ≈

1.414213562373095 * 3.141592653589793 ≈

1.414213562373095 * 3 = 4.242640687119285

1.414213562373095 * 0.141592653589793 ≈

Compute 1.414213562373095 * 0.1 = 0.1414213562373095

1.414213562373095 * 0.041592653589793 ≈

0.04 *1.414213562373095 = 0.0565685424949238

0.001592653589793 *1.414213562373095 ≈ 0.0022522017712

Total ≈ 0.0565685424949238 + 0.0022522017712 ≈ 0.0588207442661

So total for 0.141592653589793 ≈ 0.1414213562373095 +0.0588207442661 ≈ 0.2002421005034

So total sqrt(2)*π ≈ 4.242640687119285 +0.2002421005034 ≈ 4.442882787622685

Multiply by 5: 4.442882787622685 *5 ≈ 22.214413938113425

Divide by 8: 22.214413938113425 /8 ≈ 2.776801742264178

Rounded to 10 decimal places: 2.7768017423.

Hmm, so there's a slight difference here. Let me check with a calculator:

Using a calculator, 5*sqrt(2)*pi/8:

5 * 1.41421356237 = 7.07106781185

7.07106781185 * 3.141592653589793 ≈ 22.2144146901923

22.2144146901923 /8 ≈ 2.7768018362740375

So approximately 2.7768018363 when calculated with higher precision. So rounding to 10 decimal places: 2.7768018363. But depending on the exact calculation steps, the decimal approximation might vary slightly. However, the exact answer is (5 sqrt(2) π)/8, and the numerical approximation should be around 2.776801836.

But let me confirm with another method. Let's compute 5*sqrt(2)*pi/8:

sqrt(2) ≈ 1.4142135623730950488016887242097

pi ≈ 3.1415926535897932384626433832795

Multiply sqrt(2) and pi: 1.4142135623730950488016887242097 * 3.1415926535897932384626433832795

Using a calculator for exact multiplication:

1.4142135623730950488016887242097 × 3.1415926535897932384626433832795 ≈

Let me use a calculator:

1.414213562373095 * 3.141592653589793 ≈ 4.442882908158179

Then multiply by 5: 4.442882908158179 ×5 = 22.214414540790895

Divide by 8: 22.214414540790895 /8 = 2.7768018175988617

Rounded to 10 decimal places: 2.7768018176.

So there's a slight discrepancy due to calculator precision, but the exact value is (5√2 π)/8, and the numerical approximation is approximately 2.7768018176.

Therefore, the final answer is {"answer": "\\frac{5\\sqrt{2}\\pi}{8}", "numerical_answer": "2.7768018176"}.
</think>

{"answer": "\\frac{5\\sqrt{2}\\pi}{8}", "numerical_answer": "2.7768018176"}