Let's compute the definite integral step by step:

\[
\int_0^6 \left( x + (x-3)^7 + \sin(x-3) \right) dx
\]

We can split the integral into three parts:

1. \(\int_0^6 x \, dx\)
2. \(\int_0^6 (x-3)^7 \, dx\)
3. \(\int_0^6 \sin(x-3) \, dx\)

### 1. Compute \(\int_0^6 x \, dx\):
\[
\int x \, dx = \frac{x^2}{2} + C
\]
Evaluated from 0 to 6:
\[
\left. \frac{x^2}{2} \right|_0^6 = \frac{6^2}{2} - \frac{0^2}{2} = 18
\]

### 2. Compute \(\int_0^6 (x-3)^7 \, dx\):
Let \( u = x - 3 \), then \( du = dx \). When \( x = 0 \), \( u = -3 \), and when \( x = 6 \), \( u = 3 \). The integral becomes:
\[
\int_{-3}^3 u^7 \, du
\]
Since \( u^7 \) is an odd function and the limits are symmetric about 0, the integral is 0:
\[
\int_{-3}^3 u^7 \, du = 0
\]

### 3. Compute \(\int_0^6 \sin(x-3) \, dx\):
Again, let \( u = x - 3 \), so \( du = dx \). The integral becomes:
\[
\int_{-3}^3 \sin(u) \, du
\]
The antiderivative of \(\sin(u)\) is \(-\cos(u)\), so:
\[
\left. -\cos(u) \right|_{-3}^3 = -\cos(3) - (-\cos(-3)) = -\cos(3) + \cos(3) = 0
\]
(Note: \(\cos(-3) = \cos(3)\) because cosine is even.)

### Summing the results:
\[
18 + 0 + 0 = 18
\]

### Numerical approximation:
The exact answer is 18, so the numerical approximation is simply 18.0000000000.

### Final answer in JSON format:
```json
{"answer": "18", "numerical_answer": "18.0000000000"}
```