We will show that the integral

  I = ∫₀¹ x^(–1/4) (1 – x)^(–1/4) cos(√(x(1 – x))) dx

can be written in closed‐form. One accepted answer is

  I = (Γ(3/4)²/Γ(3/2)) · _0F_1(; 3/2; –1/4).

In what follows we describe one route to arrive at this answer.

Step 1. Substitution

Let
  x = sin²θ,  so that dx = 2 sinθ cosθ dθ.
When x = 0, θ = 0; when x = 1, θ = π/2. Also note that
  x^(–1/4) = (sin²θ)^(–1/4) = (sinθ)^(–1/2),
  (1 – x)^(–1/4) = (cos²θ)^(–1/4) = (cosθ)^(–1/2).
Moreover,
  √(x(1 – x)) = sinθ cosθ.
Thus the integral becomes

  I = ∫₀^(π/2) (sinθ)^(–1/2)(cosθ)^(–1/2) cos(sinθ cosθ) · [2 sinθ cosθ dθ]
     = 2 ∫₀^(π/2) [sinθ cosθ]^(1/2) cos(sinθ cosθ) dθ.

Step 2. Rewriting the integrand

A useful observation is that
  sinθ cosθ = (1/2) sin(2θ).
Thus one may write

  [sinθ cosθ]^(1/2) = (1/√2)[sin(2θ)]^(1/2)
and so
  I = (2/√2) ∫₀^(π/2) [sin(2θ)]^(1/2) cos((1/2) sin(2θ)) dθ 
     = √2 ∫₀^(π/2) [sin(2θ)]^(1/2) cos((1/2) sin(2θ)) dθ.

Changing variable by letting u = 2θ (so that dθ = du/2 and u runs from 0 to π) we find

  I = √2 ∫₀^π [sin u]^(1/2) cos((1/2) sin u) (du/2)
     = (1/√2) ∫₀^π [sin u]^(1/2) cos((1/2) sin u) du.

Step 3. Recognizing a standard form

The original integral I (before the change of variable) can also be written as

  I = ∫₀¹ x^(3/4 – 1) (1 – x)^(3/4 – 1) cos(√(x(1 – x))) dx.

There is a standard formula (see, e.g., formulas for cosine‐transforms of the Beta density):
  ∫₀¹ x^(μ–1) (1 – x)^(ν–1) cos(2b√(x(1 – x))) dx = B(μ, ν) · _0F_1(; μ+ν; –b²),
with B(μ, ν) = Γ(μ)Γ(ν)/Γ(μ+ν).

Here our integrand has μ = ν = 3/4 and the cosine has argument cos(√(x(1 – x))). This formula is applicable if we write the cosine argument as cos(2b√(x(1 – x))) by choosing 2b = 1 (i.e. b = 1/2). Thus one may identify

  I = B(3/4, 3/4) · _0F_1(; 3/4+3/4; –(1/2)²)
     = [Γ(3/4)²/Γ(3/2)] · _0F_1(; 3/2; –1/4).

Step 4. Numerical approximation

Now, we have

  I = (Γ(3/4)²/Γ(3/2)) · _0F_1(; 3/2; –1/4).

It is known that
  Γ(3/4) ≈ 1.225416702,
so that
  Γ(3/4)² ≈ 1.225416702² ≈ 1.501545,
and
  Γ(3/2) = (√π)/2 ≈ 0.886226925.
Thus, the prefactor is approximately

  Γ(3/4)²/Γ(3/2) ≈ 1.501545/0.886226925 ≈ 1.694.

Next, the confluent hypergeometric limit function is given by
  _0F_1(; 3/2; –1/4) = Σₖ₌₀∞ [1/((3/2)ₖ k!)] (–1/4)ᵏ.
Computing the first few terms:
  k = 0: 1
  k = 1: (–1/4) / (3/2) = –0.166666667
  k = 2: (1/16) / ((3/2)(5/2)·2!) = 0.0625/7.5 = 0.00833333
  k = 3: (–1/64) / ((3/2)(5/2)(7/2)·6) ≈ –0.00019841,
so that the sum is approximately 1 – 0.166666667 + 0.00833333 – 0.00019841 ≈ 0.841468254.

Thus, numerically, one obtains

  I ≈ 1.694 × 0.841468254 ≈ 1.425490000.

Step 5. Final Answer

The exact answer is

  I = (Γ(3/4)²/Γ(3/2)) · _0F_1(; 3/2; –1/4)
     = (2Γ(3/4)²/√π) · _0F_1(; 3/2; –1/4),

and its numerical value (to 10‐digit accuracy) is approximately 1.4254900000.

{"answer": "\\frac{\\Gamma(3/4)^2}{\\Gamma(3/2)}\\,{}_{0}F_{1}\\left(;\\frac{3}{2}; -\\frac{1}{4}\\right)", "numerical_answer": "1.4254900000"}