To solve the definite integral \(\int\limits_0^1 \frac{1}{\sqrt{1+x}} \mathbf{K}\left(\sqrt{\frac{x}{1+x}}\right) \mathbf{K}\left(\sqrt{1-x}\right) dx\), we need to carefully analyze the integrand and use known properties of the complete elliptic integral of the first kind, \(\mathbf{K}(k)\).

### Step 1: Analytical Computation

The complete elliptic integral of the first kind is defined as:
\[
\mathbf{K}(k) = \int_0^{\frac{\pi}{2}} \frac{1}{\sqrt{1 - k^2 \sin^2 \theta}} \, d\theta
\]

Given the integrand:
\[
\frac{1}{\sqrt{1+x}} \mathbf{K}\left(\sqrt{\frac{x}{1+x}}\right) \mathbf{K}\left(\sqrt{1-x}\right)
\]

We recognize that \(\mathbf{K}\left(\sqrt{\frac{x}{1+x}}\right)\) and \(\mathbf{K}\left(\sqrt{1-x}\right)\) are complete elliptic integrals of the first kind with specific arguments.

### Step 2: Simplification and Known Results

We use the following known result for the product of two complete elliptic integrals:
\[
\mathbf{K}(k) \mathbf{K}(\sqrt{1-k^2}) = \frac{\pi^2}{4}
\]

In our case, let \(k = \sqrt{\frac{x}{1+x}}\). Then:
\[
\sqrt{1 - k^2} = \sqrt{1 - \frac{x}{1+x}} = \sqrt{\frac{1}{1+x}} = \frac{1}{\sqrt{1+x}}
\]

Thus:
\[
\mathbf{K}\left(\sqrt{\frac{x}{1+x}}\right) \mathbf{K}\left(\sqrt{1 - \frac{x}{1+x}}\right) = \mathbf{K}\left(\sqrt{\frac{x}{1+x}}\right) \mathbf{K}\left(\frac{1}{\sqrt{1+x}}\right)
\]

Using the known result:
\[
\mathbf{K}\left(\sqrt{\frac{x}{1+x}}\right) \mathbf{K}\left(\sqrt{1 - \frac{x}{1+x}}\right) = \frac{\pi^2}{4}
\]

### Step 3: Integral Evaluation

The integral simplifies to:
\[
\int_0^1 \frac{1}{\sqrt{1+x}} \cdot \frac{\pi^2}{4} \, dx = \frac{\pi^2}{4} \int_0^1 \frac{1}{\sqrt{1+x}} \, dx
\]

We now evaluate the remaining integral:
\[
\int_0^1 \frac{1}{\sqrt{1+x}} \, dx
\]

Let \(u = 1 + x\), then \(du = dx\) and the limits change from \(x = 0\) to \(u = 1\) and \(x = 1\) to \(u = 2\):
\[
\int_1^2 \frac{1}{\sqrt{u}} \, du = \int_1^2 u^{-\frac{1}{2}} \, du = \left[ 2u^{\frac{1}{2}} \right]_1^2 = 2\sqrt{2} - 2
\]

Thus, the integral evaluates to:
\[
\frac{\pi^2}{4} \left(2\sqrt{2} - 2\right) = \frac{\pi^2}{2} (\sqrt{2} - 1)
\]

### Step 4: Numerical Approximation

We now compute the numerical approximation of the result:
\[
\frac{\pi^2}{2} (\sqrt{2} - 1) \approx \frac{9.869604401}{2} \times (1.414213562 - 1) \approx 4.934802201 \times 0.414213562 \approx 2.044822751
\]

### Final Answer

\[
\boxed{
\begin{aligned}
\text{"answer": "}\frac{\pi^2}{2} (\sqrt{2} - 1)\text{"}, \\
\text{"numerical_answer": "2.044822751"}
\end{aligned}
}
\]