
To solve the definite integral \(\int_0^1 x^{-1/4}(1-x)^{1/4}\left[1 - \sqrt{x(1-x)}\right]^{-2} \, dx\), we proceed with the following steps:


### Step 1: Substitution to Simplify the Integrand
Let \( u = \sqrt{\frac{x}{1-x}} \), which implies \( x = \frac{u^2}{1+u^2} \) and \( dx = \frac{2u}{(1+u^2)^2} \, du \). Under this substitution:
- \( x(1-x) = \frac{u^2}{(1+u^2)^2} \), so \( \sqrt{x(1-x)} = \frac{u}{1+u^2} \).
- The denominator becomes \( \left[1 - \frac{u}{1+u^2}\right]^2 = \left(\frac{u^2 - u + 1}{1+u^2}\right)^2 \).
- \( x^{-1/4} = \left(\frac{u^2}{1+u^2}\right)^{-1/4} = \frac{(1+u^2)^{1/4}}{u^{1/2}} \).
- \( (1-x)^{1/4} = \left(\frac{1}{1+u^2}\right)^{1/4} = \frac{1}{(1+u^2)^{1/4}} \).

Combining these, the integrand simplifies to:
\[
x^{-1/4}(1-x)^{1/4} \cdot \frac{1}{\left[1 - \sqrt{x(1-x)}\right]^2} \cdot dx = \frac{2u^{1/2}}{(u^2 - u + 1)^2} \, du
\]

### Step 2: Adjusting the Limits of Integration
As \( x \to 0 \), \( u \to 0 \); as \( x \to 1 \), \( u \to \infty \). Thus, the integral transforms to:
\[
\int_0^\infty \frac{2u^{1/2}}{(u^2 - u + 1)^2} \, du
\]


### Step 3: Further Simplification Using \( t = \sqrt{u} \)
Let \( t = \sqrt{u} \), so \( u = t^2 \) and \( du = 2t \, dt \). The integral becomes:
\[
4 \int_0^\infty \frac{t^2}{(t^4 - t^2 + 1)^2} \, dt
\]

### Step 4: Leveraging Symmetry and Beta Function
Using the identity \( t^4 - t^2 + 1 = \frac{t^6 + 1}{t^2 + 1} \), we rewrite the denominator as \( \left(\frac{t^6 + 1}{t^2 + 1}\right)^2 \). The integral then simplifies to:
\[
4 \int_0^\infty \frac{t^2 (t^2 + 1)^2}{(t^6 + 1)^2} \, dt
\]

Expanding and splitting the integrand, we use properties of the Beta function and Gamma function to evaluate the resulting integrals. After simplification, the integral reduces to \( \pi \).


### Numerical Approximation
The exact value of the integral is \( \pi \), which approximates to \( 3.1415926536 \) when rounded to 10 decimal places.


{"answer": "\(\pi\)", "numerical_answer": "3.1415926536"}