Let's start by analyzing the integral:
\[
I = \int_{64}^{729} \frac{x^{1/2}}{x^{1/2} - x^{1/3}} \, dx
\]

**Step 1: Simplify the integrand**

Rewrite numerator and denominator:
\[
\frac{x^{1/2}}{x^{1/2} - x^{1/3}} = \frac{1}{1 - x^{-1/6}}
\]
To see this, factor \(x^{1/2}\) from the denominator:
\[
x^{1/2} - x^{1/3} = x^{1/2} \left(1 - x^{-1/6}\right)
\]
So
\[
\frac{x^{1/2}}{x^{1/2} - x^{1/3}} = \frac{x^{1/2}}{x^{1/2} (1 - x^{-1/6})} = \frac{1}{1 - x^{-1/6}}
\]

**Step 2: Substitute \(u = x^{1/6}\)**

Let \(x = u^6\), so \(dx = 6u^5 du\).
Change the limits:
- When \(x=64\), \(u = 64^{1/6} = 2\).
- When \(x=729\), \(u = 729^{1/6} = 3\).

Substitute into the integral:
\[
I = \int_{x=64}^{x=729} \frac{1}{1 - x^{-1/6}} dx = \int_{u=2}^{u=3} \frac{1}{1 - u^{-1}} \cdot 6u^5 du
\]
But \(1 - u^{-1} = \frac{u-1}{u}\), so its reciprocal is \(\frac{u}{u-1}\):
\[
I = \int_{u=2}^{u=3} \frac{u}{u-1} \cdot 6u^5 du = 6 \int_{2}^{3} \frac{u^6}{u-1} du
\]

**Step 3: Expand the numerator**

Letâ€™s expand:
\[
\frac{u^6}{u-1}
\]
We perform polynomial long division:
\[
u^6 = (u-1)(u^5 + u^4 + u^3 + u^2 + u + 1) + 1
\]
So
\[
\frac{u^6}{u-1} = u^5 + u^4 + u^3 + u^2 + u + 1 + \frac{1}{u-1}
\]

**Step 4: Break up the integral**

Thus,
\[
I = 6 \int_{2}^{3} \left[u^5 + u^4 + u^3 + u^2 + u + 1 + \frac{1}{u-1}\right] du
\]

Compute each integral:

- \(\int u^n du = \frac{u^{n+1}}{n+1}\)
- \(\int \frac{1}{u-1} du = \ln|u-1|\)

So,
\[
I = 6\left[\frac{u^{6}}{6} + \frac{u^{5}}{5} + \frac{u^{4}}{4} + \frac{u^{3}}{3} + \frac{u^{2}}{2} + u + \ln|u-1| \right]_{2}^{3}
\]

**Step 5: Plug in the bounds**

Calculate at \(u=3\):
- \(3^6 = 729\)
- \(3^5 = 243\)
- \(3^4 = 81\)
- \(3^3 = 27\)
- \(3^2 = 9\)
- \(\ln(2)\)

At \(u=2\):
- \(2^6 = 64\)
- \(2^5 = 32\)
- \(2^4 = 16\)
- \(2^3 = 8\)
- \(2^2 = 4\)
- \(\ln(1) = 0\)

Evaluate each term (\(F(u)\)):
\[
F(u) = \frac{u^6}{6} + \frac{u^5}{5} + \frac{u^4}{4} + \frac{u^3}{3} + \frac{u^2}{2} + u + \ln|u-1|
\]

Compute at \(u=3\):
\[
F(3) = \frac{729}{6} + \frac{243}{5} + \frac{81}{4} + \frac{27}{3} + \frac{9}{2} + 3 + \ln 2
\]
At \(u=2\):
\[
F(2) = \frac{64}{6} + \frac{32}{5} + \frac{16}{4} + \frac{8}{3} + \frac{4}{2} + 2 + 0
\]

Take the difference:

\[
I = 6 [F(3) - F(2)]
\]

Let's keep as fractions for the exact value, but let's also compute numerically.

**Step 6: Simplify and Approximate Numerically**

First, compute each term:

At \(u=3\):
- \(\frac{729}{6} = 121.5\)
- \(\frac{243}{5} = 48.6\)
- \(\frac{81}{4} = 20.25\)
- \(\frac{27}{3} = 9\)
- \(\frac{9}{2} = 4.5\)
- \(3.0\)
- \(\ln 2 \approx 0.6931471806\)

Total sum for \(u=3\):
\[
121.5 + 48.6 + 20.25 + 9 + 4.5 + 3 + 0.6931471806 = 207.5431471806
\]

At \(u=2\):
- \(\frac{64}{6} \approx 10.6666666667\)
- \(\frac{32}{5} = 6.4\)
- \(\frac{16}{4} = 4\)
- \(\frac{8}{3} \approx 2.6666666667\)
- \(\frac{4}{2} = 2.0\)
- \(2.0\)
- \(0\)

Total sum for \(u=2\):
\[
10.6666666667 + 6.4 + 4 + 2.6666666667 + 2 + 2 = 27.7333333334
\]

Subtract:
\[
207.5431471806 - 27.7333333334 = 179.8098138472
\]
Multiply by 6:
\[
I = 6 \times 179.8098138472 = 1078.8588830832
\]
Rounded to 10 decimal places:
\[
I \approx 1078.8588830832
\]

**Step 7: Write the exact answer in LaTeX**

The exact answer is:
\[
6 \left( 
\frac{3^6}{6} + \frac{3^5}{5} + \frac{3^4}{4} + \frac{3^3}{3} + \frac{3^2}{2} + 3 + \ln 2
-
\left[
\frac{2^6}{6} + \frac{2^5}{5} + \frac{2^4}{4} + \frac{2^3}{3} + \frac{2^2}{2} + 2
\right]
\right)
\]

Now, provide the final answer in the required JSON format:

```json
{"answer": "6 \\left( \\frac{3^6}{6} + \\frac{3^5}{5} + \\frac{3^4}{4} + \\frac{3^3}{3} + \\frac{3^2}{2} + 3 + \\ln 2 - \\left[ \\frac{2^6}{6} + \\frac{2^5}{5} + \\frac{2^4}{4} + \\frac{2^3}{3} + \\frac{2^2}{2} + 2 \\right ] \\right)", "numerical_answer": "1078.8588830832"}
```