
To solve the definite integral \(\int_0^1\left(\frac{x^2}{2-x^2}+\sqrt{\frac{2x}{x+1}}\right)\:dx\), we split it into two parts: \(I_1 = \int_0^1 \frac{x^2}{2-x^2}\,dx\) and \(I_2 = \int_0^1 \sqrt{\frac{2x}{x+1}}\,dx\).

### Step 1: Compute \(I_1\)
Rewrite the integrand using algebraic manipulation:
\[
\frac{x^2}{2-x^2} = -1 + \frac{2}{2-x^2}
\]
Thus,
\[
I_1 = \int_0^1 \left(-1 + \frac{2}{2-x^2}\right) dx = \int_0^1 -1\,dx + 2\int_0^1 \frac{1}{2-x^2}\,dx
\]
The first integral is straightforward:
\[
\int_0^1 -1\,dx = -[x]_0^1 = -1
\]
For the second integral, use the standard result \(\int \frac{1}{a^2 - x^2}\,dx = \frac{1}{2a}\ln\left|\frac{a+x}{a-x}\right| + C\) with \(a = \sqrt{2}\):
\[
2\int_0^1 \frac{1}{2-x^2}\,dx = 2 \cdot \frac{1}{2\sqrt{2}} \left[\ln\left(\frac{\sqrt{2}+x}{\sqrt{2}-x}\right)\right]_0^1 = \frac{1}{\sqrt{2}} \ln\left(\frac{\sqrt{2}+1}{\sqrt{2}-1}\right)
\]
Simplify \(\frac{\sqrt{2}+1}{\sqrt{2}-1} = (\sqrt{2}+1)^2 = 3 + 2\sqrt{2}\), so:
\[
I_1 = -1 + \frac{1}{\sqrt{2}} \ln(3 + 2\sqrt{2})
\]

### Step 2: Compute \(I_2\)
Let \(t = \sqrt{\frac{2x}{x+1}}\). Then \(t^2 = \frac{2x}{x+1}\), solving for \(x\) gives \(x = \frac{t^2}{2 - t^2}\) and \(dx = \frac{4t}{(2 - t^2)^2}dt\). The limits change from \(x=0 \to t=0\) to \(x=1 \to t=1\). Thus:
\[
I_2 = \int_0^1 t \cdot \frac{4t}{(2 - t^2)^2} dt = 4 \int_0^1 \frac{t^2}{(2 - t^2)^2} dt
\]
Decompose the integrand:
\[
\frac{t^2}{(2 - t^2)^2} = \frac{1}{2 - t^2} - \frac{2}{(2 - t^2)^2}
\]
Integrate term by term. For \(\int \frac{1}{2 - t^2}dt\), use the same standard result as before. For \(\int \frac{2}{(2 - t^2)^2}dt\), use the formula \(\int \frac{1}{(a^2 - x^2)^2}dx = \frac{x}{2a^2(a^2 - x^2)} + \frac{1}{4a^3}\ln\left|\frac{a+x}{a-x}\right| + C\) with \(a = \sqrt{2}\). After simplification, the logarithmic terms cancel, leaving:
\[
I_2 = 2 - \frac{1}{\sqrt{2}} \ln(3 + 2\sqrt{2})
\]

### Step 3: Total Integral
Adding \(I_1\) and \(I_2\), the logarithmic terms cancel:
\[
I_1 + I_2 = \left(-1 + \frac{1}{\sqrt{2}} \ln(3 + 2\sqrt{2})\right) + \left(2 - \frac{1}{\sqrt{2}} \ln(3 + 2\sqrt{2})\right) = 1
\]

### Numerical Approximation
The exact value is \(1\), so the numerical approximation is \(1.0000000000\).

{"answer": "1", "numerical_answer": "1.0000000000"}