We start with the integral

  I = ∫₀∞ 1/(eˣ + 1) dx.

Step 1. Change of variable:
Let u = e^(–x) so that when x = 0, u = 1, and when x → ∞, u = 0. Then, since
  du = –e^(–x) dx  or dx = –du/u,
the integrand becomes:

  eˣ = 1/u  ⟹ 1/(eˣ+1) = 1/(1/u + 1) = u/(1+u).

Thus, substituting into the integral yields:
  I = ∫₀∞ [u/(1+u)] · (–du/u) = –∫₁⁰ (1/(1+u)) du.

Step 2. Reverse the limits:
Reversing the limits changes the sign of the integral,
  I = ∫₀¹ 1/(1+u) du.

Step 3. Evaluate the new integral:
The antiderivative of 1/(1+u) is ln|1+u|. Evaluating from 0 to 1 gives:
  I = ln|1+u| ∣ from 0 to 1 = ln(2) – ln(1) = ln 2.

Step 4. Numerical approximation:
  ln 2 ≈ 0.6931471806.

Thus, the final answers are:

{"answer": "\\ln 2", "numerical_answer": "0.6931471806"}