Let's solve the integral step by step:

\[
I = \int_{\frac{1}{4}}^4 \frac{\tan^{-1}(x)}{x} dx
\]

### Step 1: Analytical Solution

First, recall the integral representation:
\[
\int \frac{\tan^{-1}(x)}{x} dx
\]
Let's use Feynman's trick (differentiation under the integral sign):

Let
\[
F(a) = \int_0^a \frac{\tan^{-1}(x)}{x} dx
\]
But we need from \(\frac{1}{4}\) to \(4\), so first, we seek an antiderivative.

#### Find an antiderivative

Let’s use integration by parts:

Let \(u = \tan^{-1}(x)\), \(dv = \frac{dx}{x}\).

Then:
\[
du = \frac{dx}{1 + x^2}
\]
\[
v = \ln x
\]

By integration by parts:
\[
\int \frac{\tan^{-1}(x)}{x}\,dx = \tan^{-1}(x)\ln x - \int \ln x \cdot \frac{dx}{1 + x^2}
\]
So:
\[
I = \int_{\frac{1}{4}}^4 \frac{\tan^{-1}(x)}{x} dx
= \left[\tan^{-1}(x)\ln x\right]_{\frac{1}{4}}^{4} - \int_{\frac{1}{4}}^{4} \frac{\ln x}{1+x^2} dx
\]

Now, let’s compute these pieces.

#### Evaluate \(\tan^{-1}(x)\ln x\) at endpoints

At \(x = 4\):

- \(\tan^{-1}(4)\)
- \(\ln 4 = 2\ln 2\)

At \(x = \frac{1}{4}\):

- \(\tan^{-1}\left(\frac{1}{4}\right)\)
- \(\ln \frac{1}{4} = -2\ln 2\)

Thus:
\[
\Big[\tan^{-1}(x) \ln x \Big]_{\frac{1}{4}}^{4} 
= \tan^{-1}(4) \cdot 2\ln 2 - \tan^{-1}\left(\frac{1}{4}\right)(-2\ln 2) 
= 2\ln 2\left[\tan^{-1}(4) + \tan^{-1}\left(\frac{1}{4}\right)\right]
\]

Recall that:
\[
\tan^{-1}(a) + \tan^{-1}\left(\frac{1}{a}\right) = \frac{\pi}{2}\quad (a > 0)
\]
Thus,
\[
\tan^{-1}(4) + \tan^{-1}\left(\frac{1}{4}\right) = \frac{\pi}{2}
\]

Therefore,
\[
\Big[\tan^{-1}(x) \ln x \Big]_{\frac{1}{4}}^{4} = 2\ln 2 \cdot \frac{\pi}{2} = \pi \ln 2
\]

#### Now handle the remaining integral:

\[
J = \int_{\frac{1}{4}}^{4} \frac{\ln x}{1 + x^2} dx
\]

Observe that:

Let’s use the substitution \(x \mapsto 1/x\):

If \(x = t,\ dx = dt\).
When \(x = \frac{1}{4}\), \(1/x = 4\).
When \(x = 4\), \(1/x = \frac{1}{4}\).

So:

\[
J = \int_{\frac{1}{4}}^4 \frac{\ln x}{1 + x^2} dx = \int_4^{\frac{1}{4}} \frac{\ln(1/t)}{1 + (1/t)^2} \cdot \left(-\frac{dt}{t^2}\right)
\]
But,
- \(\ln(1/t) = -\ln t\)
- \(1 + (1/t)^2 = 1 + 1/t^2 = (t^2 + 1)/(t^2)\)
- \(-\frac{dt}{t^2}\), and the limits are swapped from \(\frac{1}{4}\) to 4, so minus sign cancels; switch limits back.

So:

\[
= \int_{\frac{1}{4}}^{4} \frac{-\ln t}{\frac{t^2 + 1}{t^2}} \cdot \frac{1}{t^2} dt
= \int_{\frac{1}{4}}^{4} \frac{-\ln t}{t^2 + 1} dt
\]

So:

\[
J = -\int_{\frac{1}{4}}^{4} \frac{\ln x}{x^2 + 1} dx
\]
But this means:

\[
J = -J
\implies J = 0
\]

Hence,

\[
I = \pi \ln 2
\]

### Step 2: Numerical Approximation

Calculate \(\pi \ln 2\):

\[
\ln 2 \approx 0.6931471806
\]
\[
\pi \ln 2 \approx 3.1415926536 \times 0.6931471806 = 2.1775860903
\]

### Step 3: Final Answer in JSON

```json
{"answer": "\\pi\\ln 2", "numerical_answer": "2.1775860903"}
```