# Evaluating $\large\int_0^\infty\frac{\tanh(x)}{\exp(x)}dx$

## Step 1: Rewrite the integrand
Let's start by rewriting the hyperbolic tangent in terms of exponentials:

$$\tanh(x) = \frac{\sinh(x)}{\cosh(x)} = \frac{e^x - e^{-x}}{e^x + e^{-x}}$$

Now, our integral becomes:

$$\int_0^\infty\frac{\tanh(x)}{e^x}dx = \int_0^\infty\frac{1}{e^x}\cdot\frac{e^x - e^{-x}}{e^x + e^{-x}}dx = \int_0^\infty\frac{e^x - e^{-x}}{e^{2x} + 1}dx$$

## Step 2: Substitute $u = e^x$
Let's make the substitution $u = e^x$, which gives:
- $dx = \frac{du}{u}$
- When $x = 0$, $u = 1$
- When $x \to \infty$, $u \to \infty$

So our integral becomes:

$$\int_1^\infty\frac{u - \frac{1}{u}}{u^2 + 1}\cdot\frac{du}{u} = \int_1^\infty\frac{1 - \frac{1}{u^2}}{u^2 + 1}du$$

## Step 3: Split the integral
Let's split this into two parts:

$$\int_1^\infty\frac{1}{u^2 + 1}du - \int_1^\infty\frac{1}{u^2(u^2 + 1)}du$$

For the first integral, we know:
$$\int\frac{1}{u^2 + 1}du = \arctan(u) + C$$

So the first part evaluates to:
$$\left[\arctan(u)\right]_1^\infty = \frac{\pi}{2} - \arctan(1) = \frac{\pi}{2} - \frac{\pi}{4} = \frac{\pi}{4}$$

## Step 4: Evaluate the second integral
For the second integral, let's use partial fractions:

$$\frac{1}{u^2(u^2 + 1)} = \frac{A}{u} + \frac{B}{u^2} + \frac{Cu + D}{u^2 + 1}$$

Multiplying both sides by $u^2(u^2 + 1)$:
$$1 = A \cdot u(u^2 + 1) + B(u^2 + 1) + (Cu + D)u^2$$

Expanding:
$$1 = Au^3 + Au + Bu^2 + B + Cu^3 + Du^2$$

Grouping terms:
$$1 = (A+C)u^3 + (B+D)u^2 + Au + B$$

Comparing coefficients:
- $u^3$: $A+C = 0 \implies C = -A$
- $u^2$: $B+D = 0 \implies D = -B$
- $u^1$: $A = 0$
- $u^0$: $B = 1$

Thus: $A = 0$, $B = 1$, $C = 0$, $D = -1$

So we have:
$$\frac{1}{u^2(u^2 + 1)} = \frac{1}{u^2} - \frac{1}{u^2 + 1}$$

The second integral becomes:
$$\int_1^\infty\left(\frac{1}{u^2} - \frac{1}{u^2 + 1}\right)du = \left[-\frac{1}{u} - \arctan\left(\frac{1}{u}\right)\right]_1^\infty$$

At $u = 1$: $-1 - \arctan(1) = -1 - \frac{\pi}{4}$
At $u = \infty$: $0 - 0 = 0$

So the second integral equals: $1 + \frac{\pi}{4}$

## Step 5: Combine the results
Now we combine our results:
$$\frac{\pi}{4} - \left(1 + \frac{\pi}{4}\right) = -1$$

Therefore:
$$\int_0^\infty\frac{\tanh(x)}{e^x}dx = -1$$

## Numerical Approximation
The exact result is $-1$, which as a decimal is $-1.0000000000$ to 10 decimal places.

{"answer": "-1", "numerical_answer": "-1.0000000000"}