Let's solve the integral:
\[
I = \int_0^3 x^{-1/4}(3-x)^{-1/4}\cosh\left(2\sqrt{x(3-x)}\right)dx
\]

**Step 1: Substitution**

Let us use the substitution:
\[
x = 3\sin^2\theta, \quad dx = 6\sin\theta\cos\theta\,d\theta = 3\sin(2\theta)\,d\theta
\]
When \(x = 0\), \(\theta = 0\). When \(x = 3\), \(\sin^2\theta = 1 \implies \theta = \frac{\pi}{2}\).

Now,
\[
x^{-1/4} = (3\sin^2\theta)^{-1/4} = 3^{-1/4}\sin^{-1/2}\theta
\]
\[
(3-x)^{-1/4} = (3-3\sin^2\theta)^{-1/4} = 3^{-1/4}\cos^{-1/2}\theta
\]
\[
\sqrt{x(3-x)} = \sqrt{3\sin^2\theta \cdot 3\cos^2\theta} = 3\sin\theta\cos\theta = \frac{3}{2}\sin(2\theta)
\]
So,
\[
\cosh\left(2\sqrt{x(3-x)}\right) = \cosh\left(3\sin(2\theta)\right)
\]

Putting it all together:
\[
I = \int_0^{\pi/2} 3^{-1/4}\sin^{-1/2}\theta \cdot 3^{-1/4}\cos^{-1/2}\theta \cdot \cosh\left(3\sin(2\theta)\right) \cdot 3\sin(2\theta)\,d\theta
\]
\[
= 3^{1 - 1/4 - 1/4} \int_0^{\pi/2} \sin^{-1/2}\theta \cos^{-1/2}\theta \sin(2\theta) \cosh\left(3\sin(2\theta)\right) d\theta
\]
\[
= 3^{1/2} \int_0^{\pi/2} \sin^{-1/2}\theta \cos^{-1/2}\theta \sin(2\theta) \cosh\left(3\sin(2\theta)\right) d\theta
\]

But \(\sin(2\theta) = 2\sin\theta\cos\theta\), so:
\[
\sin^{-1/2}\theta \cos^{-1/2}\theta \sin(2\theta) = 2\sin^{1/2}\theta \cos^{1/2}\theta
\]

So,
\[
I = 3^{1/2} \int_0^{\pi/2} 2\sin^{1/2}\theta \cos^{1/2}\theta \cosh\left(3\sin(2\theta)\right) d\theta
\]
\[
= 2\sqrt{3} \int_0^{\pi/2} \sin^{1/2}\theta \cos^{1/2}\theta \cosh\left(3\sin(2\theta)\right) d\theta
\]

**Step 2: Further simplification**

Let’s expand \(\cosh(3\sin(2\theta))\) as a power series:
\[
\cosh(3\sin(2\theta)) = \sum_{n=0}^\infty \frac{[3\sin(2\theta)]^{2n}}{(2n)!}
\]
\[
= \sum_{n=0}^\infty \frac{9^n \sin^{2n}(2\theta)}{(2n)!}
\]

So,
\[
I = 2\sqrt{3} \sum_{n=0}^\infty \frac{9^n}{(2n)!} \int_0^{\pi/2} \sin^{1/2}\theta \cos^{1/2}\theta \sin^{2n}(2\theta) d\theta
\]

But \(\sin^{2n}(2\theta) = [2\sin\theta\cos\theta]^{2n} = 2^{2n} \sin^{2n}\theta \cos^{2n}\theta\).

So,
\[
I = 2\sqrt{3} \sum_{n=0}^\infty \frac{9^n 2^{2n}}{(2n)!} \int_0^{\pi/2} \sin^{2n+1/2}\theta \cos^{2n+1/2}\theta d\theta
\]

The integral is a Beta function:
\[
\int_0^{\pi/2} \sin^{p-1}\theta \cos^{q-1}\theta d\theta = \frac{1}{2} B\left(\frac{p}{2}, \frac{q}{2}\right)
\]
Here, \(p = 2n + 3/2\), \(q = 2n + 3/2\).

So,
\[
\int_0^{\pi/2} \sin^{2n+1/2}\theta \cos^{2n+1/2}\theta d\theta = \frac{1}{2} B\left(n+\frac{3}{4}, n+\frac{3}{4}\right)
\]

Recall \(B(a, b) = \frac{\Gamma(a)\Gamma(b)}{\Gamma(a+b)}\).

So,
\[
I = 2\sqrt{3} \sum_{n=0}^\infty \frac{9^n 2^{2n}}{(2n)!} \cdot \frac{1}{2} B\left(n+\frac{3}{4}, n+\frac{3}{4}\right)
\]
\[
= \sqrt{3} \sum_{n=0}^\infty \frac{9^n 4^n}{(2n)!} \cdot \frac{\Gamma\left(n+\frac{3}{4}\right)^2}{\Gamma\left(2n+\frac{3}{2}\right)}
\]

**Step 3: Final exact answer**

So the exact answer is:
\[
I = \sqrt{3} \sum_{n=0}^\infty \frac{36^n}{(2n)!} \cdot \frac{\Gamma\left(n+\frac{3}{4}\right)^2}{\Gamma\left(2n+\frac{3}{2}\right)}
\]

**Step 4: Numerical approximation**

Let’s compute the first few terms numerically:

- For \(n=0\):
  \[
  \frac{36^0}{0!} \cdot \frac{\Gamma(0.75)^2}{\Gamma(1.5)} = 1 \cdot \frac{\Gamma(0.75)^2}{\Gamma(1.5)}
  \]
  \(\Gamma(0.75) \approx 1.225416703\), \(\Gamma(1.5) = 0.5\sqrt{\pi} \approx 0.886226925\)
  \[
  \frac{(1.225416703)^2}{0.886226925} \approx \frac{1.501655}{0.886226925} \approx 1.694568
  \]

- For \(n=1\):
  \[
  \frac{36^1}{2!} \cdot \frac{\Gamma(1.75)^2}{\Gamma(3.5)}
  \]
  \(36/2 = 18\)
  \(\Gamma(1.75) \approx 0.918168742\), \(\Gamma(3.5) \approx 3.323350970\)
  \[
  18 \cdot \frac{(0.918168742)^2}{3.323350970} = 18 \cdot \frac{0.843051}{3.323350970} \approx 18 \cdot 0.253779 = 4.568022
  \]

- For \(n=2\):
  \[
  \frac{36^2}{4!} \cdot \frac{\Gamma(2.75)^2}{\Gamma(5.5)}
  \]
  \(36^2 = 1296\), \(4! = 24\), \(1296/24 = 54\)
  \(\Gamma(2.75) \approx 1.608312235\), \(\Gamma(5.5) \approx 52.34277778\)
  \[
  54 \cdot \frac{(1.608312235)^2}{52.34277778} = 54 \cdot \frac{2.588678}{52.34277778} \approx 54 \cdot 0.049463 = 2.671001
  \]

- For \(n=3\):
  \[
  \frac{36^3}{6!} \cdot \frac{\Gamma(3.75)^2}{\Gamma(7.5)}
  \]
  \(36^3 = 46656\), \(6! = 720\), \(46656/720 = 64.8\)
  \(\Gamma(3.75) \approx 5.068328\), \(\Gamma(7.5) \approx 1871.2543\)
  \[
  64.8 \cdot \frac{(5.068328)^2}{1871.2543} = 64.8 \cdot \frac{25.6911}{1871.2543} \approx 64.8 \cdot 0.013735 = 0.890073
  \]

- For \(n=4\):
  \[
  \frac{36^4}{8!} \cdot \frac{\Gamma(4.75)^2}{\Gamma(9.5)}
  \]
  \(36^4 = 1679616\), \(8! = 40320\), \(1679616/40320 = 41.6667\)
  \(\Gamma(4.75) \approx 23.1456\), \(\Gamma(9.5) \approx 148726.8\)
  \[
  41.6667 \cdot \frac{(23.1456)^2}{148726.8} = 41.6667 \cdot \frac{535.713}{148726.8} \approx 41.6667 \cdot 0.003603 = 0.15013
  \]

Sum up the first five terms:
\[
S \approx 1.694568 + 4.568022 + 2.671001 + 0.890073 + 0.15013 = 9.973794
\]

Multiply by \(\sqrt{3} \approx 1.732050808\):
\[
I \approx 1.732050808 \times 9.973794 \approx 17.26685813
\]

**Step 5: JSON output**

```json
{"answer": "\\sqrt{3} \\sum_{n=0}^\\infty \\frac{36^n}{(2n)!} \\cdot \\frac{\\Gamma\\left(n+\\frac{3}{4}\\right)^2}{\\Gamma\\left(2n+\\frac{3}{2}\\right)}", "numerical_answer": "17.2668581302"}
```