
To solve the definite integral \(\int_0^\infty \frac{\sin\sqrt{3}\,x - \sin\frac{x}{\sqrt{3}}}{x} e^{-x^2}\, dx\), we proceed as follows:


### Step 1: Split the Integral
The integrand can be split into two terms:
\[
\int_0^\infty \frac{\sin\sqrt{3}\,x - \sin\frac{x}{\sqrt{3}}}{x} e^{-x^2}\, dx = \int_0^\infty \frac{\sin\sqrt{3}\,x}{x} e^{-x^2}\, dx - \int_0^\infty \frac{\sin\frac{x}{\sqrt{3}}}{x} e^{-x^2}\, dx.
\]
Let \(a = \sqrt{3}\) and \(b = \frac{1}{\sqrt{3}}\). We denote the two integrals as \(I_1 = \int_0^\infty \frac{\sin a x}{x} e^{-x^2}\, dx\) and \(I_2 = \int_0^\infty \frac{\sin b x}{x} e^{-x^2}\, dx\), so the original integral is \(I = I_1 - I_2\).


### Step 2: Evaluate \(I_1\) and \(I_2\) Using Differentiation Under the Integral Sign
Consider the function \(F(t) = \int_0^\infty \frac{\sin t x}{x} e^{-x^2}\, dx\). Differentiating \(F(t)\) with respect to \(t\) gives:
\[
F'(t) = \int_0^\infty \cos(t x) e^{-x^2}\, dx.
\]
The integral \(\int_0^\infty \cos(t x) e^{-x^2}\, dx\) is a standard Gaussian integral. For even functions, \(\int_{-\infty}^\infty \cos(t x) e^{-x^2}\, dx = \sqrt{\pi} e^{-t^2/4}\), so:
\[
\int_0^\infty \cos(t x) e^{-x^2}\, dx = \frac{\sqrt{\pi}}{2} e^{-t^2/4}.
\]
Integrating \(F'(t)\) from \(0\) to \(t\) (with \(F(0) = 0\)) gives:
\[
F(t) = \int_0^t \frac{\sqrt{\pi}}{2} e^{-s^2/4}\, ds.
\]
Using the substitution \(u = s/2\), this becomes:
\[
F(t) = \sqrt{\pi} \int_0^{t/2} e^{-u^2}\, du = \frac{\pi}{2} \cdot \frac{2}{\sqrt{\pi}} \int_0^{t/2} e^{-u^2}\, du = \frac{\pi}{2} \, \text{erf}\left(\frac{t}{2}\right),
\]
where \(\text{erf}(z)\) is the error function.


### Step 3: Apply to \(I_1\) and \(I_2\)
For \(I_1\) with \(t = a = \sqrt{3}\):
\[
I_1 = \frac{\pi}{2} \, \text{erf}\left(\frac{\sqrt{3}}{2}\right).
\]
For \(I_2\) with \(t = b = \frac{1}{\sqrt{3}}\):
\[
I_2 = \frac{\pi}{2} \, \text{erf}\left(\frac{1}{2\sqrt{3}}\right) = \frac{\pi}{2} \, \text{erf}\left(\frac{\sqrt{3}}{6}\right).
\]


### Step 4: Combine Results
The original integral is:
\[
I = \frac{\pi}{2} \left( \text{erf}\left(\frac{\sqrt{3}}{2}\right) - \text{erf}\left(\frac{\sqrt{3}}{6}\right) \right).
\]


### Step 5: Numerical Approximation
Using numerical values for the error function:
- \(\text{erf}\left(\frac{\sqrt{3}}{2}\right) \approx 0.770668012285\)
- \(\text{erf}\left(\frac{\sqrt{3}}{6}\right) \approx 0.316712416872\)

Thus:
\[
I \approx \frac{\pi}{2} \left( 0.770668012285 - 0.316712416872 \right) \approx \frac{\pi}{2} \cdot 0.453955595413 \approx 0.7130712800.
\]


{"answer": "\\frac{\\pi}{2} \\left( \\text{erf}\\left(\\frac{\\sqrt{3}}{2}\\right) - \\text{erf}\\left(\\frac{\\sqrt{3}}{6}\\right) \\right)", "numerical_answer": "0.7130712800"}