

To solve the definite integral \(\int_{1}^{\infty} (x^2 - 1)^{3/2} e^{-x^2/4} H_5\left(\frac{x}{2}\right) \, dx\), we proceed as follows:

### Step 1: Simplify the Hermite Polynomial
The Hermite polynomial \(H_5(z)\) is given by \(H_5(z) = 32z^5 - 160z^3 + 120z\). Substituting \(z = \frac{x}{2}\), we get:
\[
H_5\left(\frac{x}{2}\right) = 32\left(\frac{x}{2}\right)^5 - 160\left(\frac{x}{2}\right)^3 + 120\left(\frac{x}{2}\right) = x^5 - 20x^3 + 60x.
\]

### Step 2: Substitute \(t = x^2\)
Let \(t = x^2\), so \(x = \sqrt{t}\) and \(dx = \frac{dt}{2\sqrt{t}}\). The integral transforms to:
\[
\int_{1}^{\infty} (t - 1)^{3/2} e^{-t/4} \left(t^{5/2} - 20t^{3/2} + 60t^{1/2}\right) \cdot \frac{dt}{2\sqrt{t}}.
\]
Simplifying the polynomial term:
\[
\frac{t^{5/2} - 20t^{3/2} + 60t^{1/2}}{2\sqrt{t}} = \frac{t^2 - 20t + 60}{2}.
\]
Thus, the integral becomes:
\[
\frac{1}{2} \int_{1}^{\infty} (t - 1)^{3/2} e^{-t/4} (t^2 - 20t + 60) \, dt.
\]

### Step 3: Substitute \(u = t - 1\)
Let \(u = t - 1\), so \(t = u + 1\) and \(dt = du\). The integral transforms to:
\[
\frac{1}{2} e^{-1/4} \int_{0}^{\infty} u^{3/2} e^{-u/4} \left((u + 1)^2 - 20(u + 1) + 60\right) \, du.
\]
Expanding the polynomial:
\[
(u + 1)^2 - 20(u + 1) + 60 = u^2 - 18u + 41.
\]

### Step 4: Evaluate the Integral Using Gamma Functions
The integral splits into three terms involving gamma functions:
\[
\int_{0}^{\infty} u^{3/2} e^{-u/4} (u^2 - 18u + 41) \, du = \int_{0}^{\infty} u^{7/2} e^{-u/4} \, du - 18 \int_{0}^{\infty} u^{5/2} e^{-u/4} \, du + 41 \int_{0}^{\infty} u^{3/2} e^{-u/4} \, du.
\]
Using the gamma function identity \(\int_{0}^{\infty} u^s e^{-au} \, du = \frac{\Gamma(s + 1)}{a^{s + 1}}\), we compute each term:
- First term: \(\Gamma\left(\frac{9}{2}\right) \cdot 4^{9/2} = 3360\sqrt{\pi}\)
- Second term: \(-18 \cdot \Gamma\left(\frac{7}{2}\right) \cdot 4^{7/2} = -4320\sqrt{\pi}\)
- Third term: \(41 \cdot \Gamma\left(\frac{5}{2}\right) \cdot 4^{5/2} = 984\sqrt{\pi}\)

Summing these terms gives \(24\sqrt{\pi}\). Thus, the integral simplifies to:
\[
\frac{1}{2} e^{-1/4} \cdot 24\sqrt{\pi} = 12 e^{-1/4} \sqrt{\pi}.
\]

### Step 5: Numerical Approximation
Using \(e^{-1/4} \approx 0.7788007830714049\) and \(\sqrt{\pi} \approx 1.7724538509055159\), we compute:
\[
12 \cdot 0.7788007830714049 \cdot 1.7724538509055159 \approx 16.5646642324.
\]

### Final Answer
{"answer": "12 e^{-\\frac{1}{4}} \\sqrt{\\pi}", "numerical_answer": "16.5646642324"}