We wish to evaluate

  I = ∫₀¹ (x⁶ + x⁴ + x²)·√(2x⁴ + 3x² + 6) dx.

A good strategy is to “guess” an antiderivative and then verify it by differentiation. In our case, one may try an antiderivative of the form

  F(x) = A·x³ · (2x⁴ + 3x² + 6)^(3/2).

We will show that with the proper choice of constant A the derivative F′(x) reproduces the given integrand.

Step 1. Let S = 2x⁴ + 3x² + 6. Then
  F(x) = A·x³ S^(3/2).
Differentiate using the product and chain rules:
  F′(x) = A [ d/dx (x³)·S^(3/2) + x³·d/dx (S^(3/2)) ].
Since d/dx (x³) = 3x² and
  d/dx (S^(3/2)) = (3/2) S^(1/2)·S′,
we first compute S′:
  S = 2x⁴ + 3x² + 6 → S′ = 8x³ + 6x.
Thus,
  F′(x) = A [ 3x² S^(3/2) + x³·(3/2) S^(1/2)(8x³ + 6x) ]
      = A S^(1/2) [ 3x² S + (3/2)x³(8x³ + 6x) ]
      = A S^(1/2) [ 3x² (2x⁴ + 3x² + 6) + (3/2)x³ (8x³+6x) ].

Let us simplify the term coming from the second part:
  (3/2)x³ (8x³ + 6x) = (3/2)[8x⁶ + 6x⁴] = 12x⁶ + 9x⁴.

Now also expand the first part:
  3x² (2x⁴ + 3x² + 6) = 6x⁶ + 9x⁴ + 18x².

Thus,
  F′(x) = A S^(1/2)[ (6x⁶ + 9x⁴ + 18x²) + (12x⁶ + 9x⁴) ]
      = A S^(1/2)[ 18x⁶ + 18x⁴ + 18x² ]
      = 18A · x² (x⁴ + x² + 1) · S^(1/2).

We want F′(x) to equal the given integrand
  (x⁶ + x⁴ + x²)·√S.
But note that
  x⁶ + x⁴ + x² = x² (x⁴ + x² + 1).
Thus, if we choose A such that
  18A = 1 ⟹ A = 1/18,
then
  F′(x) = x² (x⁴+x²+1) S^(1/2)
which is exactly our integrand.

Step 2. Therefore, an antiderivative is
  F(x) = (1/18)·x³·(2x⁴ + 3x² + 6)^(3/2).

The definite integral from 0 to 1 is then

  I = F(1) – F(0).

At x = 1:
  F(1) = (1/18)·1³·(2·1⁴ + 3·1² + 6)^(3/2)
     = (1/18)·(2 + 3 + 6)^(3/2)
     = (1/18)·(11)^(3/2) = (11^(3/2))/18.

At x = 0, note x³ = 0 so F(0)= 0.

Thus, the exact answer is

  I = (11^(3/2))/18 = (11√11)/18.

Step 3. For a numerical approximation, note:
  √11 ≈ 3.31662479036  ⟹  11√11 ≈ 36.4828726940.
Then,
  I ≈ 36.4828726940 / 18 ≈ 2.0268262619.

Step 4. We now output the answer in the requested JSON format.

{"answer": "\\frac{11\\sqrt{11}}{18}", "numerical_answer": "2.0268262619"}