We wish to evaluate

  I = ∫₁∞ x (x² – 1²)^(2 – 3/2) e^(–(0.5)² x²) H₍₂*2₎(0.5 x) dx.

Step 1. Simplify the integrand

(a) The exponent in (x²–1²)^(2–3/2):
  2 – 3/2 = 1/2,
so (x² – 1)^(1/2) = √(x² – 1).

(b) The exponential: (0.5)² = 0.25 so e^(–0.25 x²).

(c) The Hermite polynomial H₍₂*2₎(0.5 x) is H₄(0.5 x). In the “physicist’s” convention the Hermite polynomial H₄(z) is given by
  H₄(z) = 16z⁴ – 48z² + 12.
Thus, substituting z = 0.5 x we have
  H₄(0.5 x) = 16 (0.5 x)⁴ – 48 (0.5 x)² + 12
           = 16 (x⁴/16) – 48 (x²/4) + 12
           = x⁴ – 12x² + 12.

Thus the integrand becomes
  x √(x² – 1) e^(–x²/4) (x⁴ –12x² + 12).

So the integral is

  I = ∫₁∞ e^(–x²/4)[x⁵ – 12x³ + 12x] √(x² – 1) dx.

Step 2. Change of variable

A good substitution is to let
  u = x² – 1  → du = 2x dx  ⟹  x dx = du/2.
Also, note that √(x² – 1) = √u and x² = u + 1. In addition,
  x⁴ = (x²)² = (u + 1)².
The polynomial factor becomes:
  x⁵ – 12x³ + 12x = x (x⁴ – 12x² + 12)
     = x [ (u + 1)² – 12(u + 1) + 12 ]
Expand:
  (u + 1)² – 12(u + 1) + 12 = u² + 2u + 1 – 12u – 12 + 12
              = u² – 10u + 1.
Also, the exponential becomes
  e^(–x²/4) = e^(–(u + 1)/4) = e^(–1/4)e^(–u/4).

Since x dx = du/2, the limits change: when x = 1 we have u = 0, and when x → ∞, u → ∞.

Thus the integral becomes
  I = ∫₍u=0₎∞ e^(–(u+1)/4)[x (x⁴ –12x²+12)] √u · (dx)
But replacing x dx by du/2 (remember the factor x in the integrand has been used already to cancel dx) we obtain
  I = (1/2) e^(–1/4) ∫₀∞ e^(–u/4)(u² – 10u + 1) √u du.

Step 3. Express the u–integral in terms of Gamma functions

Write the integral as
  J = ∫₀∞ u^(1/2) e^(–u/4)(u² – 10u + 1) du.
Break this into three integrals:
  J = ∫₀∞ u^(5/2) e^(–u/4) du – 10∫₀∞ u^(3/2) e^(–u/4) du + ∫₀∞ u^(1/2) e^(–u/4) du.
Recall the Gamma integral:
  ∫₀∞ u^(ν–1)e^(–λu) du = Γ(ν)/λ^(ν).
Identify:
• For u^(5/2): Write exponent as 5/2 = (7/2 – 1) so ν = 7/2, λ = 1/4. This gives
  ∫₀∞ u^(5/2) e^(–u/4) du = Γ(7/2) / (1/4)^(7/2) = Γ(7/2) · 4^(7/2).
• For u^(3/2): Here ν = 5/2, so the integral equals
  Γ(5/2) · 4^(5/2).
• For u^(1/2): Here ν = 3/2, so the integral equals
  Γ(3/2) · 4^(3/2).

Thus
  J = 4^(7/2)Γ(7/2) – 10·4^(5/2)Γ(5/2) + 4^(3/2)Γ(3/2).

Recall that
  4^(3/2) = 8, 4^(5/2) = 32, 4^(7/2) = 128.
Also, the Gamma values:
  Γ(3/2) = (√π)/2,
  Γ(5/2) = (3√π)/4,
  Γ(7/2) = (5/2)·Γ(5/2) = (5/2)·(3√π/4) = (15√π)/8.
Now substitute:
  J = 128·(15√π/8) – 10·32·(3√π/4) + 8·(√π/2)
Compute each term:
• 128·(15√π/8) = 16·15√π = 240√π,
• 10·32·(3√π/4) = 10·8·3√π = 240√π,
• 8·(√π/2) = 4√π.
Thus
  J = 240√π – 240√π + 4√π = 4√π.

Returning to I:
  I = (1/2)e^(–1/4) J = (1/2)e^(–1/4)(4√π) = 2√π e^(–1/4).

Step 4. Numerical Approximation

We have:
  √π ≈ 1.772453850905516 and e^(–1/4) ≈ 0.7788007830714049.
Thus,
  2√π e^(–1/4) ≈ 2 * 1.772453850905516 * 0.7788007830714049 ≈ 2.7621680443.

Final Answer in JSON format:

{"answer": "$2\\sqrt{\\pi}e^{-\\frac{1}{4}}$", "numerical_answer": "2.7621680443"}