<think>
Okay, let's see. I need to compute the definite integral of arcsin(x) times arccos(x) from 0 to 1. Hmm, both arcsin and arccos are inverse trigonometric functions, and their product might have some relationship that I can exploit. Let me start by recalling some properties of these functions.

First, I remember that arcsin(x) + arccos(x) equals π/2. That's a key identity. Maybe I can use that to simplify the product. Let me write that down: arcsin(x) = π/2 - arccos(x). So, if I let u = arcsin(x), then arccos(x) would be π/2 - u. But I'm not sure if substitution is the way to go here. Alternatively, maybe integration by parts would work since we have a product of two functions.

Integration by parts formula is ∫u dv = uv - ∫v du. Let me choose which part to set as u and which as dv. Let's try letting u = arcsin(x) and dv = arccos(x) dx. Then du would be 1/√(1 - x²) dx, and I need to find v by integrating dv. Wait, integrating arccos(x) dx. Let me recall: the integral of arccos(x) dx is x arccos(x) - √(1 - x²) + C. Let me check that derivative. If I take d/dx [x arccos(x) - √(1 - x²)], that's arccos(x) + x*(-1/√(1 - x²)) - (1/(2√(1 - x²)))*(-2x). Simplifying, that's arccos(x) - x/√(1 - x²) + x/√(1 - x²) = arccos(x). So yes, that's correct. So v = x arccos(x) - √(1 - x²).

So applying integration by parts: uv - ∫v du. So that's [arcsin(x)(x arccos(x) - √(1 - x²))] from 0 to 1 minus the integral from 0 to 1 of (x arccos(x) - √(1 - x²)) * (1/√(1 - x²)) dx.

Let me compute the first part, the evaluated terms. Let's plug in x=1 and x=0.

At x=1: arcsin(1) is π/2. Then, x arccos(x) is 1 * arccos(1) = 1*0 = 0. Then, √(1 - 1²) = 0. So the term at x=1 is π/2 * (0 - 0) = 0.

At x=0: arcsin(0) is 0. The term is 0*(0 arccos(0) - √(1 - 0)) = 0. So the entire evaluated part is 0 - 0 = 0. So the first part is 0.

Now, the remaining part is -∫ from 0 to 1 of (x arccos(x) - √(1 - x²)) / √(1 - x²) dx. Let me split that into two integrals: - [∫x arccos(x)/√(1 - x²) dx - ∫√(1 - x²)/√(1 - x²) dx] from 0 to 1.

Simplifying the second integral: √(1 - x²)/√(1 - x²) is 1, so ∫1 dx from 0 to 1 is just 1. So the integral becomes - [∫x arccos(x)/√(1 - x²) dx - 1]. So that's -∫x arccos(x)/√(1 - x²) dx + 1.

Now, the remaining integral is ∫x arccos(x)/√(1 - x²) dx from 0 to 1. Let me focus on that. Let me make a substitution here. Let t = arccos(x). Then, dt/dx = -1/√(1 - x²), so -dt = dx/√(1 - x²). Also, x = cos(t). When x=0, t=π/2; when x=1, t=0.

So substituting, the integral becomes ∫ (from t=π/2 to t=0) cos(t) * t / √(1 - cos²(t)) * (-dt). Wait, let's see. The original integral is x arccos(x) / √(1 - x²) dx. So x is cos(t), arccos(x) is t, dx is -√(1 - x²) dt? Wait, maybe I need to check substitution again.

Wait, if t = arccos(x), then x = -√(1 - x²) dt. Wait, no. Let me re-express. If t = arccos(x), then dt/dx = -1/√(1 - x²). So dx = -√(1 - x²) dt. But in the integral, we have x arccos(x) / √(1 - x²) dx. So substituting x = cos(t), arccos(x) = t, dx = -√(1 - cos²(t)) dt. But √(1 - cos²(t)) is sin(t). So dx = -sin(t) dt. So substituting into the integral:

∫ [cos(t) * t / sin(t)] * (-sin(t) dt) from t=π/2 to 0. The sin(t) in the denominator and the sin(t) from dx cancel out. The negative sign flips the limits of integration. So the integral becomes ∫ from 0 to π/2 of cos(t) * t dt.

So that's ∫0^{π/2} t cos(t) dt. Hmm, this seems manageable. Let's compute this integral. Again, integration by parts. Let me set u = t, dv = cos(t) dt. Then du = dt, v = sin(t). So integration by parts gives uv - ∫v du = t sin(t) - ∫ sin(t) dt from 0 to π/2.

Compute that: t sin(t) evaluated from 0 to π/2 minus ∫ sin(t) dt from 0 to π/2. The first term is [ (π/2) sin(π/2) - 0*sin(0) ] = π/2 * 1 = π/2. The integral of sin(t) is -cos(t), so evaluated from 0 to π/2: -cos(π/2) + cos(0) = -0 + 1 = 1. So the integral becomes π/2 - 1.

So going back, the integral ∫x arccos(x)/√(1 - x²) dx from 0 to 1 is equal to π/2 - 1. Therefore, the previous expression was - [ (π/2 - 1) ] + 1. Wait, let's retrace.

Original integral after substitution: the integral was - [ ∫x arccos(x)/√(1 - x²) dx - 1 ] = - [ (π/2 - 1) - 1 ]? Wait, no. Wait, the integral ∫x arccos(x)/√(1 - x²) dx from 0 to1 is equal to π/2 -1. So then the expression is - (π/2 -1) +1. So that's -π/2 +1 +1 = -π/2 +2.

So putting it all together, the original integral is equal to 0 (from the first part) plus (- (π/2 -1) +1 ), which is 2 - π/2. Wait, the original integral was ∫ arcsin(x) arccos(x) dx from 0 to1, which after integration by parts became 0 - [ ∫x arccos(x)/√(1 - x²) dx -1 ] = - [ (π/2 -1) -1 ] = -π/2 +1 +1 = 2 - π/2.

Wait, let me check again. The integral after by parts was - [ integral - 1 ]. So the integral was - integral +1. The integral was (π/2 -1). So - (π/2 -1) +1 = -π/2 +1 +1 = 2 - π/2. So the final result is 2 - π/2.

Wait, but let me verify this. Let me compute 2 - π/2. Since π is approximately 3.1415926536, so π/2 is about 1.5707963268. Then 2 - 1.5707963268 ≈ 0.4292036732. Let me check if that's correct numerically. Alternatively, maybe I made a mistake in the steps.

Alternatively, let me consider another approach. Since arcsin(x) + arccos(x) = π/2, so perhaps we can express the product arcsin(x)arccos(x) in terms of (π/2 - arccos(x)) arccos(x) = π/2 arccos(x) - (arccos(x))^2. Then integrate from 0 to1. So ∫0^1 [π/2 arccos(x) - (arccos(x))^2 ] dx. Maybe that's easier.

Let me try that. Let me split the integral into two parts: π/2 ∫ arccos(x) dx - ∫ (arccos(x))^2 dx from 0 to1.

First integral: ∫ arccos(x) dx. We know that integral is x arccos(x) - √(1 - x²) + C. Evaluated from 0 to1. At x=1: 1*0 - 0 =0. At x=0: 0*π/2 -1 = -1. So the integral is 0 - (-1) =1. So π/2 *1 = π/2.

Second integral: ∫ (arccos(x))^2 dx from 0 to1. Let me compute this. Let me use substitution. Let t = arccos(x), so x = cos(t), dx = -sin(t) dt. When x=0, t=π/2; x=1, t=0. So the integral becomes ∫ (t)^2 * (-sin(t) dt) from π/2 to0. Flipping the limits: ∫0^{π/2} t^2 sin(t) dt. Wait, t squared times sin(t). So integrate t² sin(t) dt. Integration by parts. Let u = t², dv = sin(t) dt. Then du = 2t dt, v = -cos(t). So uv - ∫v du = -t² cos(t) + ∫2t cos(t) dt.

Now, the remaining integral is 2∫t cos(t) dt. Again, integration by parts. Let u = t, dv = cos(t) dt. Then du = dt, v = sin(t). So 2[ t sin(t) - ∫ sin(t) dt ] = 2[ t sin(t) + cos(t) ].

Putting it all together: the integral of t² sin(t) dt is -t² cos(t) + 2t sin(t) + 2 cos(t) + C. Evaluated from 0 to π/2.

At π/2: - (π/2)^2 * cos(π/2) + 2*(π/2)*sin(π/2) + 2 cos(π/2) = - (π²/4)*0 + 2*(π/2)*1 + 2*0 = π.

At 0: -0^2 * cos(0) + 2*0*sin(0) + 2 cos(0) = 0 +0 +2*1=2.

So the integral from 0 to π/2 is π - 2. Therefore, the integral ∫ (arccos(x))^2 dx from 0 to1 is π -2.

So going back to the original split: π/2 *1 - (π -2) = π/2 - π +2 = -π/2 +2. Which is the same result as before. So the integral is 2 - π/2. So that's the exact answer. So the exact answer is 2 - π/2.

Now, the numerical approximation. Let's compute 2 - π/2. π is approximately 3.141592653589793. So π/2 is 1.5707963267948966. Then 2 - 1.5707963267948966 = 0.4292036732051034. Rounded to 10 decimal places, that's 0.4292036732.

So the final answer is 2 - π/2, which in LaTeX is 2 - \frac{\pi}{2}, and the numerical approximation is approximately 0.4292036732.
</think>

{"answer": "2 - \\frac{\\pi}{2}", "numerical_answer": "0.4292036732"}