# Evaluating $\intop_0^2 x^{1/2}(2-x)^{1/2}\cosh\left(1\sqrt{x(2-x)}\right)dx$

I'll approach this definite integral by exploring the structure and making appropriate substitutions.

## Step 1: Analyze the integral

Let's first examine the integrand $x^{1/2}(2-x)^{1/2}\cosh\left(1\sqrt{x(2-x)}\right)$. 

Notice that the integrand contains the term $\sqrt{x(2-x)}$ which suggests a symmetry about $x = 1$. 

## Step 2: Make a substitution

Let's set $u = \sqrt{x(2-x)}$. This implies:
- When $x = 0$, $u = 0$
- When $x = 2$, $u = 0$
- When $x = 1$, $u = 1$ (maximum value)

To express $x$ in terms of $u$, I'll solve:
$u^2 = x(2-x) = 2x - x^2$
$x^2 - 2x + u^2 = 0$

Using the quadratic formula:
$x = \frac{2 \pm \sqrt{4-4u^2}}{2} = 1 \pm \sqrt{1-u^2}$

For $0 \leq x \leq 1$, we use $x = 1 - \sqrt{1-u^2}$
For $1 \leq x \leq 2$, we use $x = 1 + \sqrt{1-u^2}$

## Step 3: Calculate $dx$ in terms of $du$

Differentiating $u = \sqrt{x(2-x)}$ with respect to $x$:
$\frac{du}{dx} = \frac{(2-x) - x}{2\sqrt{x(2-x)}} = \frac{2-2x}{2\sqrt{x(2-x)}} = \frac{1-x}{\sqrt{x(2-x)}}$

Therefore:
$dx = \frac{\sqrt{x(2-x)}}{1-x}du$

## Step 4: Rewrite the integral with the substitution

The original integral is:
$\intop_0^2 x^{1/2}(2-x)^{1/2}\cosh\left(1\sqrt{x(2-x)}\right)dx$

Note that $\sqrt{x}\cdot\sqrt{2-x} = \sqrt{x(2-x)}$, so our integral becomes:
$\intop_0^2 \sqrt{x(2-x)}\cosh\left(\sqrt{x(2-x)}\right)dx$

Substituting $u = \sqrt{x(2-x)}$:
$\intop_0^1 u \cdot \cosh(u) \cdot \frac{\sqrt{x(2-x)}}{1-x}du \cdot 2$

The factor of 2 comes from integrating from $x=0$ to $x=2$, which corresponds to going from $u=0$ to $u=1$ and back.

Now I need to express $\frac{\sqrt{x(2-x)}}{1-x}$ in terms of $u$.

## Step 5: Simplify the substitution

Since $u = \sqrt{x(2-x)}$ and $x = 1 - \sqrt{1-u^2}$ for the first half:
$\frac{\sqrt{x(2-x)}}{1-x} = \frac{u}{\sqrt{1-u^2}}$

So our integral becomes:
$\intop_0^1 u \cdot \cosh(u) \cdot \frac{u}{\sqrt{1-u^2}}du \cdot 2 = 2\intop_0^1 \frac{u^2 \cosh(u)}{\sqrt{1-u^2}}du$

## Step 6: Further simplification

Using the identity $u^2 = 1-(1-u^2)$:
$2\intop_0^1 \frac{u^2 \cosh(u)}{\sqrt{1-u^2}}du = 2\intop_0^1 \frac{[1-(1-u^2)] \cosh(u)}{\sqrt{1-u^2}}du$
$= 2\intop_0^1 \frac{\cosh(u)}{\sqrt{1-u^2}}du - 2\intop_0^1 \frac{(1-u^2) \cosh(u)}{\sqrt{1-u^2}}du$
$= 2\intop_0^1 \frac{\cosh(u)}{\sqrt{1-u^2}}du - 2\intop_0^1 \sqrt{1-u^2} \cosh(u)du$

## Step 7: Evaluate these integrals

For the first integral, let $u = \sin\theta$, which gives $du = \cos\theta d\theta$ and $\sqrt{1-u^2} = \cos\theta$.
$2\intop_0^1 \frac{\cosh(u)}{\sqrt{1-u^2}}du = 2\intop_0^{\pi/2} \frac{\cosh(\sin\theta)}{\cos\theta}\cos\theta d\theta = 2\intop_0^{\pi/2} \cosh(\sin\theta)d\theta$

For the second integral, similarly:
$2\intop_0^1 \sqrt{1-u^2} \cosh(u)du = 2\intop_0^{\pi/2} \cos\theta \cosh(\sin\theta) \cos\theta d\theta = 2\intop_0^{\pi/2} \cos^2\theta \cosh(\sin\theta)d\theta$

## Step 8: Use special function representations

These integrals involve Bessel functions. Using standard integral representations:
$\intop_0^{\pi/2} \cosh(z\sin\theta)d\theta = \frac{\pi}{2}I_0(z)$
$\intop_0^{\pi/2} \cos^2\theta \cosh(z\sin\theta)d\theta = \frac{\pi}{4}[I_0(z) + I_1(z)]$

where $I_0$ and $I_1$ are modified Bessel functions of the first kind.

So our integral equals:
$2 \cdot \frac{\pi}{2}I_0(1) - 2 \cdot \frac{\pi}{4}[I_0(1) + I_1(1)] = \pi I_0(1) - \frac{\pi}{2}[I_0(1) + I_1(1)] = \frac{\pi}{2}[I_0(1) - I_1(1)]$

## Step 9: Evaluate the final result

The exact answer is:
$\frac{\pi}{2}[I_0(1) - I_1(1)]$

The numerical values are:
- $I_0(1) \approx 1.2660658777520084$
- $I_1(1) \approx 0.5651591039924850$

Therefore:
$\frac{\pi}{2}[I_0(1) - I_1(1)] \approx \frac{\pi}{2} \cdot [1.2660658777520084 - 0.5651591039924850] \approx \frac{\pi}{2} \cdot 0.7009067737595234 \approx 1.1011581566606675$

Rounding to 10 decimal places: 1.1011581567

{"answer": "\\frac{\\pi}{2}[I_0(1) - I_1(1)]", "numerical_answer": "1.1011581567"}