We wish to evaluate

  I = ∫₀^(π/4) arctan((1 + tan x)/√2) dx.

Step 1. Use a substitution to reveal symmetry.
Let u = π/4 – x. Then,
  x = π/4 – u  and  dx = –du,
and the limits transform as:
  when x = 0, u = π/4,
  when x = π/4, u = 0.
Thus,
  I = ∫₍u=π/4₎^(0) arctan((1 + tan(π/4 – u))/√2) (–du)
    = ∫₀^(π/4) arctan((1 + tan(π/4 – u))/√2) du.

Step 2. Simplify the integrand.
Recall the tangent subtraction formula:
  tan(π/4 – u) = (tan(π/4) – tan u)/(1 + tan(π/4)tan u).
Since tan(π/4) = 1, this becomes:
  tan(π/4 – u) = (1 – tan u)/(1 + tan u).
Then,
  1 + tan(π/4 – u) = 1 + (1 – tan u)/(1 + tan u)
    = ( (1 + tan u) + (1 – tan u) )/(1 + tan u)
    = (2)/(1 + tan u).
Therefore, the integrand becomes:
  arctan((1 + tan(π/4 – u))/√2) = arctan(2/(√2 (1 + tan u)))
    = arctan(√2/(1 + tan u)).

Thus, we obtain a second representation for I:
  I = ∫₀^(π/4) arctan(√2/(1 + tan u)) du.

Step 3. Add the two representations.
Let
  I₁ = ∫₀^(π/4) arctan((1 + tan x)/√2) dx  and
  I₂ = ∫₀^(π/4) arctan(√2/(1 + tan x)) dx.
We have shown that I₁ = I₂ = I. Now, add them:
  I₁ + I₂ = ∫₀^(π/4) [ arctan((1 + tan x)/√2) + arctan(√2/(1 + tan x)) ] dx.

Step 4. Use the arctan sum formula.
For any positive a, it holds that
  arctan(a) + arctan(1/a) = π/2.
Here, let a = (1 + tan x)/√2. Since tan x ≥ 0 for x ∈ [0, π/4], a > 0, so:
  arctan((1 + tan x)/√2) + arctan(√2/(1 + tan x)) = π/2.
Thus,
  I₁ + I₂ = ∫₀^(π/4) (π/2) dx = (π/2)·(π/4) = π²/8.

Since I₁ = I₂ = I, we have:
  2I = π²/8  ⟹  I = π²/16.

Step 5. Numerical approximation.
We approximate π²/16 ≈ (9.869604401089358)/16 ≈ 0.6168502751.

The final answer is:

{"answer": "$\\frac{\\pi^2}{16}$", "numerical_answer": "0.6168502751"}