To solve the definite integral \(\int\limits_{0}^{2} H_{3}\left(\sqrt{x(2-x)}\right) dx\), we need to understand the function \(H_{3}(y)\). The Hermite polynomial \(H_{3}(y)\) is given by:

\[ H_{3}(y) = 8y^3 - 12y \]

Thus, the integral becomes:

\[ \int\limits_{0}^{2} H_{3}\left(\sqrt{x(2-x)}\right) dx = \int\limits_{0}^{2} \left(8\left(\sqrt{x(2-x)}\right)^3 - 12\sqrt{x(2-x)}\right) dx \]

Let's simplify the integrand:

\[ \left(\sqrt{x(2-x)}\right)^3 = \left(x(2-x)\right)^{3/2} \]
\[ \sqrt{x(2-x)} = (x(2-x))^{1/2} \]

So the integral becomes:

\[ \int\limits_{0}^{2} \left(8(x(2-x))^{3/2} - 12(x(2-x))^{1/2}\right) dx \]

We can split this into two separate integrals:

\[ 8 \int\limits_{0}^{2} (x(2-x))^{3/2} dx - 12 \int\limits_{0}^{2} (x(2-x))^{1/2} dx \]

Let's solve each integral separately.

### Integral 1: \(\int\limits_{0}^{2} (x(2-x))^{3/2} dx\)

We use the substitution \(u = x(2-x)\). Then \(du = (2 - 2x) dx\), and \(dx = \frac{du}{2(1 - x)}\).

When \(x = 0\), \(u = 0\). When \(x = 2\), \(u = 0\).

However, this substitution is not straightforward. Instead, we use a trigonometric substitution. Let \(x = 2 \sin^2 \theta\). Then \(dx = 4 \sin \theta \cos \theta d\theta\).

When \(x = 0\), \(\theta = 0\). When \(x = 2\), \(\theta = \frac{\pi}{2}\).

\[ x(2-x) = 2 \sin^2 \theta (2 - 2 \sin^2 \theta) = 4 \sin^2 \theta \cos^2 \theta \]

So the integral becomes:

\[ \int\limits_{0}^{\pi/2} (4 \sin^2 \theta \cos^2 \theta)^{3/2} \cdot 4 \sin \theta \cos \theta d\theta \]
\[ = \int\limits_{0}^{\pi/2} 64 \sin^3 \theta \cos^3 \theta \cdot 4 \sin \theta \cos \theta d\theta \]
\[ = 256 \int\limits_{0}^{\pi/2} \sin^4 \theta \cos^4 \theta d\theta \]

Using the double-angle identities, \(\sin^2 \theta = \frac{1 - \cos 2\theta}{2}\) and \(\cos^2 \theta = \frac{1 + \cos 2\theta}{2}\):

\[ \sin^4 \theta \cos^4 \theta = \left(\frac{1 - \cos 2\theta}{2}\right)^2 \left(\frac{1 + \cos 2\theta}{2}\right)^2 \]
\[ = \frac{1}{16} (1 - \cos 2\theta)^2 (1 + \cos 2\theta)^2 \]
\[ = \frac{1}{16} (1 - \cos^2 2\theta)^2 \]
\[ = \frac{1}{16} \sin^4 2\theta \]

So the integral becomes:

\[ 256 \cdot \frac{1}{16} \int\limits_{0}^{\pi/2} \sin^4 2\theta d\theta \]
\[ = 16 \int\limits_{0}^{\pi/2} \sin^4 2\theta d\theta \]

Using the reduction formula for \(\sin^4 \theta\):

\[ \int \sin^4 \theta d\theta = \frac{3}{8} \theta - \frac{1}{4} \sin 2\theta + \frac{1}{32} \sin 4\theta + C \]

So:

\[ 16 \int\limits_{0}^{\pi/2} \sin^4 2\theta d\theta = 16 \left[ \frac{3}{8} \theta - \frac{1}{4} \sin 2\theta + \frac{1}{32} \sin 4\theta \right]_0^{\pi/2} \]
\[ = 16 \left[ \frac{3}{8} \cdot \frac{\pi}{2} - 0 + 0 \right] \]
\[ = 16 \cdot \frac{3\pi}{16} \]
\[ = 3\pi \]

### Integral 2: \(\int\limits_{0}^{2} (x(2-x))^{1/2} dx\)

Using the same substitution \(x = 2 \sin^2 \theta\):

\[ \int\limits_{0}^{\pi/2} (4 \sin^2 \theta \cos^2 \theta)^{1/2} \cdot 4 \sin \theta \cos \theta d\theta \]
\[ = \int\limits_{0}^{\pi/2} 4 \sin \theta \cos \theta \cdot 4 \sin \theta \cos \theta d\theta \]
\[ = 16 \int\limits_{0}^{\pi/2} \sin^2 \theta \cos^2 \theta d\theta \]
\[ = 16 \cdot \frac{1}{16} \int\limits_{0}^{\pi/2} \sin^2 2\theta d\theta \]
\[ = \int\limits_{0}^{\pi/2} \sin^2 2\theta d\theta \]

Using the reduction formula for \(\sin^2 \theta\):

\[ \int \sin^2 \theta d\theta = \frac{1}{2} \theta - \frac{1}{4} \sin 2\theta + C \]

So:

\[ \int\limits_{0}^{\pi/2} \sin^2 2\theta d\theta = \left[ \frac{1}{2} \theta - \frac{1}{4} \sin 2\theta \right]_0^{\pi/2} \]
\[ = \frac{1}{2} \cdot \frac{\pi}{2} - 0 \]
\[ = \frac{\pi}{4} \]

### Combining the Results

\[ 8 \cdot 3\pi - 12 \cdot \frac{\pi}{4} \]
\[ = 24\pi - 3\pi \]
\[ = 21\pi \]

### Numerical Approximation

\[ 21\pi \approx 65.97344572538566 \]

### Final Answer

```json
{"answer": "21\\pi", "numerical_answer": "65.9734457254"}
```