To solve the definite integral \(\int\limits_{0}^{1} x^{-1/2} \cos\left(2\sqrt{x(1-x)}\right) dx\), we will follow the steps outlined:

### Step 1: Analytical Solution

First, let's make a substitution to simplify the integral. Let \( t = \sqrt{x} \). Then \( x = t^2 \) and \( dx = 2t \, dt \). The limits of integration change as follows:
- When \( x = 0 \), \( t = 0 \).
- When \( x = 1 \), \( t = 1 \).

Substituting these into the integral, we get:
\[
\int\limits_{0}^{1} x^{-1/2} \cos\left(2\sqrt{x(1-x)}\right) dx = \int\limits_{0}^{1} (t^2)^{-1/2} \cos\left(2\sqrt{t^2(1-t^2)}\right) \cdot 2t \, dt
\]

Simplifying the integrand:
\[
(t^2)^{-1/2} = t^{-1}
\]
\[
\sqrt{t^2(1-t^2)} = t \sqrt{1-t^2}
\]

Thus, the integral becomes:
\[
\int\limits_{0}^{1} t^{-1} \cos\left(2t \sqrt{1-t^2}\right) \cdot 2t \, dt = 2 \int\limits_{0}^{1} \cos\left(2t \sqrt{1-t^2}\right) \, dt
\]

Next, let \( u = 2t \sqrt{1-t^2} \). Then \( du = 2 \left( \sqrt{1-t^2} - \frac{t^2}{\sqrt{1-t^2}} \right) dt \). Simplifying \( du \):
\[
du = 2 \left( \frac{1 - 2t^2}{\sqrt{1-t^2}} \right) dt
\]

This substitution is not straightforward, so let's consider another approach. Notice that the integrand \(\cos\left(2\sqrt{x(1-x)}\right)\) is symmetric around \( x = \frac{1}{2} \). This suggests that we might use a trigonometric substitution.

Let \( x = \sin^2 \theta \). Then \( dx = 2 \sin \theta \cos \theta \, d\theta \). The limits of integration change as follows:
- When \( x = 0 \), \( \theta = 0 \).
- When \( x = 1 \), \( \theta = \frac{\pi}{2} \).

Substituting these into the integral, we get:
\[
\int\limits_{0}^{1} x^{-1/2} \cos\left(2\sqrt{x(1-x)}\right) dx = \int\limits_{0}^{\pi/2} (\sin^2 \theta)^{-1/2} \cos\left(2\sqrt{\sin^2 \theta (1 - \sin^2 \theta)}\right) \cdot 2 \sin \theta \cos \theta \, d\theta
\]

Simplifying the integrand:
\[
(\sin^2 \theta)^{-1/2} = \csc \theta
\]
\[
\sqrt{\sin^2 \theta (1 - \sin^2 \theta)} = \sin \theta \cos \theta
\]

Thus, the integral becomes:
\[
\int\limits_{0}^{\pi/2} \csc \theta \cos(2 \sin \theta \cos \theta) \cdot 2 \sin \theta \cos \theta \, d\theta = 2 \int\limits_{0}^{\pi/2} \cos(2 \sin \theta \cos \theta) \cos \theta \, d\theta
\]

This integral is still complex, but we recognize that it involves a Bessel function of the first kind. Specifically, the integral can be expressed in terms of the Bessel function \( J_0 \):
\[
\int\limits_{0}^{\pi/2} \cos(2 \sin \theta \cos \theta) \cos \theta \, d\theta = \frac{\pi}{2} J_0(1)
\]

Thus, the integral evaluates to:
\[
2 \cdot \frac{\pi}{2} J_0(1) = \pi J_0(1)
\]

### Step 2: Numerical Approximation

Using the known value of the Bessel function \( J_0(1) \approx 0.7651976865579666 \), we get:
\[
\pi J_0(1) \approx 3.141592653589793 \times 0.7651976865579666 \approx 2.402738984337351
\]

### Step 3: Final Answer in JSON Format

\[
\boxed{
\begin{aligned}
&\text{"answer": "\pi J_0(1)",} \\
&\text{"numerical_answer": "2.4027389843"}
\end{aligned}
}
\]