Given the integral:
\[
I = \int_0^\infty \frac{\{x\}^{\lceil x\rceil}}{1+\lceil x\rceil}\, dx
\]
where \(\{x\} = x - \lfloor x \rfloor\) is the fractional part and \(\lceil x \rceil\) is the ceiling function.

### Step 1: Break the Integral into Intervals

On each interval \(n-1 < x < n\) (\(n = 1,2,3,\dots\)):
- \(\lceil x \rceil = n\),
- \(\{x\} = x - (n-1)\) for \(x \in (n-1,n)\).

So, partition the integral:
\[
I = \sum_{n=1}^\infty \int_{n-1}^n \frac{(x-n+1)^n}{n+1} dx
\]

Now, perform the substitution \(t = x-n+1\), so \(x = t+n-1\), when \(x=n-1\), \(t=0\); when \(x=n\), \(t=1\):

So the integral over each interval becomes:
\[
\int_{n-1}^n \frac{(x-n+1)^n}{n+1} dx = \frac{1}{n+1} \int_0^1 t^n dt = \frac{1}{n+1} \cdot \frac{1}{n+1} = \frac{1}{(n+1)^2}
\]

### Step 2: Sum the Series

Therefore,
\[
I = \sum_{n=1}^{\infty} \frac{1}{(n+1)^2}
\]
Letâ€™s change variable: let \(k = n+1\), so as \(n = 1,2,3,\dots\), \(k = 2,3,4,\dots\):

\[
I = \sum_{k=2}^{\infty} \frac{1}{k^2}
\]
But
\[
\sum_{k=1}^\infty \frac{1}{k^2} = \zeta(2) = \frac{\pi^2}{6}
\]
so
\[
\sum_{k=2}^\infty \frac{1}{k^2} = \zeta(2) - 1 = \frac{\pi^2}{6} - 1
\]

### Step 3: Final Answers

The exact answer:
\[
I = \frac{\pi^2}{6} - 1
\]

Numerical approximation:
\[
I \approx \frac{9.8696044011}{6} - 1 \approx 1.644934068 - 1 = 0.6449340680
\]

### JSON Output
```json
{"answer": "\\frac{\\pi^2}{6} - 1", "numerical_answer": "0.6449340680"}
```