

To solve the definite integral \(\int_0^1 (x^6 + x^4 + x^2) \cdot \sqrt{2x^4 + 3x^2 + 6} \, dx\), we proceed with the following steps:

### Step 1: Substitution \(t = x^2\)
Let \(t = x^2\), so \(x = \sqrt{t}\) and \(dx = \frac{1}{2\sqrt{t}} dt\). When \(x = 0\), \(t = 0\); when \(x = 1\), \(t = 1\). Rewrite the integrand in terms of \(t\):
- \(x^6 = t^3\), \(x^4 = t^2\), \(x^2 = t\), so \(x^6 + x^4 + x^2 = t^3 + t^2 + t = t(t^2 + t + 1)\).
- The square root term becomes \(\sqrt{2t^2 + 3t + 6}\).

The integral transforms to:
\[
\int_0^1 t(t^2 + t + 1) \cdot \sqrt{2t^2 + 3t + 6} \cdot \frac{1}{2\sqrt{t}} dt
\]
Simplify \(t / \sqrt{t} = \sqrt{t}\), so the integrand becomes:
\[
\frac{1}{2} \int_0^1 (t^2 + t + 1) \cdot \sqrt{t(2t^2 + 3t + 6)} dt
\]
Note \(t(2t^2 + 3t + 6) = 2t^3 + 3t^2 + 6t\), so the integral is:
\[
\frac{1}{2} \int_0^1 (t^2 + t + 1) \cdot \sqrt{2t^3 + 3t^2 + 6t} dt
\]

### Step 2: Substitution \(u = 2t^3 + 3t^2 + 6t\)
Let \(u = 2t^3 + 3t^2 + 6t\). Then \(du/dt = 6t^2 + 6t + 6 = 6(t^2 + t + 1)\), so \((t^2 + t + 1) dt = du/6\). Substituting into the integral:
\[
\frac{1}{2} \int \sqrt{u} \cdot \frac{du}{6} = \frac{1}{12} \int u^{1/2} du
\]

### Step 3: Integrate and Evaluate
Integrate \(u^{1/2}\):
\[
\frac{1}{12} \cdot \frac{2}{3} u^{3/2} + C = \frac{1}{18} u^{3/2} + C
\]
Substitute back \(u = 2t^3 + 3t^2 + 6t\) and \(t = x^2\), so \(u = 2x^6 + 3x^4 + 6x^2\). Evaluate from \(x = 0\) to \(x = 1\):
- At \(x = 1\): \(u = 2(1)^6 + 3(1)^4 + 6(1)^2 = 11\), so \(\frac{1}{18} (11)^{3/2}\).
- At \(x = 0\): \(u = 0\), so \(\frac{1}{18} (0)^{3/2} = 0\).

Thus, the integral evaluates to \(\frac{11\sqrt{11}}{18}\).

### Numerical Approximation
\(\sqrt{11} \approx 3.3166247904\), so \(11\sqrt{11} \approx 36.4828726944\). Dividing by 18 gives approximately \(2.0268262608\).

{"answer": "\\frac{11\\sqrt{11}}{18}", "numerical_answer": "2.0268262608"}