Let's compute the integral:
\[
I = \int_{-\infty}^\infty e^{-2x^2-5x-3}\,dx
\]

**Step 1: Simplify the exponent**

Rewrite the exponent:
\[
-2x^2-5x-3 = -2(x^2 + \frac{5}{2}x) - 3
\]
Complete the square for \(x^2 + \frac{5}{2}x\):

\[
x^2 + \frac{5}{2}x = \left(x + \frac{5}{4}\right)^2 - \frac{25}{16}
\]
So,
\[
-2(x^2 + \frac{5}{2}x) = -2\left[\left(x + \frac{5}{4}\right)^2 - \frac{25}{16}\right] = -2\left(x + \frac{5}{4}\right)^2 + \frac{25}{8}
\]
Now combine with \(-3\):
\[
-2x^2-5x-3 = -2\left(x + \frac{5}{4}\right)^2 + \frac{25}{8} - 3
= -2\left(x + \frac{5}{4}\right)^2 + \frac{25-24}{8}
= -2\left(x + \frac{5}{4}\right)^2 + \frac{1}{8}
\]

So,
\[
I = \int_{-\infty}^\infty e^{-2\left(x+\frac{5}{4}\right)^2 + \frac{1}{8}}\,dx
= e^{1/8} \int_{-\infty}^{\infty} e^{-2\left(x+\frac{5}{4}\right)^2} dx
\]

**Step 2: Recognize the Gaussian Integral Form**

Use the substitution \(u = x + \frac{5}{4}\):
\[
I = e^{1/8} \int_{-\infty}^\infty e^{-2u^2} du
\]
The Gaussian integral:
\[
\int_{-\infty}^\infty e^{-a u^2} du = \sqrt{\frac{\pi}{a}}
\]
Here, \(a = 2\):
\[
\int_{-\infty}^\infty e^{-2u^2} du = \sqrt{\frac{\pi}{2}}
\]

**Thus:**
\[
I = e^{1/8} \sqrt{\frac{\pi}{2}}
\]

**Step 3: Numerical Approximation**

Calculate each part:

- \(e^{1/8} = e^{0.125} \approx 1.1331484531\)
- \(\sqrt{\frac{\pi}{2}} = \sqrt{1.5707963268} \approx 1.2533141373\)

So,
\[
I \approx 1.1331484531 \times 1.2533141373 \approx 1.4219123944
\]

**Step 4: Final Answer in JSON**

```json
{"answer": "e^{1/8} \\sqrt{\\frac{\\pi}{2}}", "numerical_answer": "1.4219123944"}
```