<think>
Okay, so I need to compute the definite integral from 0 to 1 of (x - 1)/[(x + 1)ln x] dx. Hmm, let's start by understanding the integrand. The function is (x - 1) divided by (x + 1) times the natural logarithm of x. The limits are from 0 to 1. 

First, I should check if there are any points where the integrand is undefined. Well, ln x approaches negative infinity as x approaches 0 from the right, and at x=1, ln x is 0. So the denominator becomes zero at x=1, which might be a point of concern. Also, at x=0, the denominator is (0 + 1)*ln 0, which is 1*(-inf), so the denominator is -infinity there. So the integrand has singularities at both endpoints. I need to check if the integral converges.

But before that, maybe there's a substitution or a trick to evaluate this integral analytically. Let me think. The integrand has x in both numerator and denominator, and a logarithm. Maybe substitution t = something related to x. Let's see. The presence of ln x suggests that substitution t = ln x might be useful, but let's try that.

Let t = ln x. Then dt = (1/x) dx, so dx = x dt. But x = e^t. So dx = e^t dt. Then, when x approaches 0, t approaches -infinity, and when x approaches 1, t approaches 0. So the integral becomes:

Integral from t = -infty to t=0 of [ (e^t - 1)/(e^t + 1) * t ] * e^t dt. Wait, let me check that substitution again.

Original integrand: (x -1)/[(x +1) ln x] dx. Substitute x = e^t, so dx = e^t dt. Then the integrand becomes (e^t -1)/(e^t +1) * (1/t) * e^t dt. Wait, because ln x = t, so 1/ln x is 1/t. So putting it all together:

(e^t -1)/(e^t +1) * (1/t) * e^t dt. Hmm, that seems a bit complicated, but maybe simplifying the numerator. Let's see:

(e^t -1)/(e^t +1) * e^t = [e^t(e^t -1)]/(e^t +1) = [e^{2t} - e^t]/(e^t +1). Not sure if that helps. Maybe split the numerator? Let's see:

Alternatively, perhaps another substitution. Let me think. The integrand (x -1)/( (x +1) ln x ). Maybe consider substitution u = x, but not sure. Alternatively, maybe integrating by parts. Let's see. Let me set u = (x -1)/(x +1), dv = dx/ln x. Then du would be [ (1)(x +1) - (x -1)(1) ]/(x +1)^2 dx = [ (x +1 -x +1 )/(x +1)^2 ] dx = 2/(x +1)^2 dx. And v would be the integral of 1/ln x dx, which is not sure. The integral of 1/ln x dx is the logarithmic integral, which is a special function, but maybe that's not helpful here. So integrating by parts might not be the way to go.

Alternatively, maybe consider expanding the numerator. Let's see, (x -1) = (x +1 -2), so (x -1)/(x +1) = 1 - 2/(x +1). So the integrand becomes [1 - 2/(x +1)] / ln x. So the integral becomes integral from 0 to1 of [1/ln x - 2/( (x +1) ln x ) ] dx. Hmm, but splitting the integral into two parts: integral of 1/ln x dx minus 2 times integral of 1/( (x +1) ln x ) dx. But the first integral, integral of 1/ln x dx, is again the logarithmic integral, which is not elementary. So maybe this approach isn't helpful.

Wait, but maybe there's a substitution that can relate the integral to a known form. Let me think. The integrand (x -1)/[(x +1) ln x]. Let me consider substitution t = (1 - x)/(1 + x), or something similar. Let's try substitution t = (1 - x)/(1 + x). Then x = (1 - t)/(1 + t). Let's compute dx. dx/dt = [ - (1 + t) - (1 - t) ]/(1 + t)^2 = [ - (1 + t +1 - t) ]/(1 + t)^2 = -2/(1 + t)^2. So dx = -2/(1 + t)^2 dt. Now, when x approaches 0, t approaches 1, and when x approaches 1, t approaches 0. So the limits would be from t=1 to t=0, but with the negative sign, it becomes from 0 to1. Let's substitute into the integrand:

Original integrand: (x -1)/[(x +1) ln x] dx. Substitute x = (1 - t)/(1 + t). Then x -1 = (1 - t - (1 + t))/(1 + t) = (-2t)/(1 + t). x +1 = (1 - t +1 + t)/(1 + t) = 2/(1 + t). So (x -1)/(x +1) = (-2t)/(1 + t) * (1 + t)/2 = -t. Then ln x = ln[(1 - t)/(1 + t)] = ln(1 - t) - ln(1 + t). So the integrand becomes:

(-t) / [ ln(1 - t) - ln(1 + t) ] * [ -2/(1 + t)^2 ] dt. Let's simplify the signs. The first term is -t, multiplied by the denominator, and then multiplied by -2/(1 + t)^2. So the negatives cancel, and we have:

[ t / ( ln(1 - t) - ln(1 + t) ) ] * [ 2/(1 + t)^2 ] dt. Let's write the denominator as ln[(1 - t)/(1 + t)]. So the integrand becomes:

t / [ ln( (1 - t)/(1 + t) ) ] * 2/(1 + t)^2 dt. Hmm, not sure if that's helpful yet. Let's see if we can manipulate the denominator. Let me note that ln( (1 - t)/(1 + t) ) = -2 artanh t, since artanh t = (1/2) ln( (1 + t)/(1 - t) ). So ln( (1 - t)/(1 + t) ) = -2 artanh t. Therefore, the integrand becomes:

t / ( -2 artanh t ) * 2/(1 + t)^2 dt. The 2 and -2 cancel, giving -t/( artanh t ) * 1/(1 + t)^2 dt. So the integral becomes:

Integral from t=0 to t=1 of [ -t/( artanh t ) * 1/(1 + t)^2 ] dt. Hmm, not sure if that's better. Maybe another substitution here. Let me think. Let me set u = artanh t. Then t = tanh u, and dt = sech^2 u du. Let's try that. Then when t=0, u=0, and when t=1, u approaches infinity. So the integral becomes:

Integral from u=0 to u=∞ of [ - tanh u / u * 1/(1 + tanh u)^2 * sech^2 u ] du. Let's simplify the terms. First, 1 + tanh u = (cosh u + sinh u)/cosh u = e^u / cosh u. So (1 + tanh u)^2 = e^{2u} / cosh^2 u. Then 1/(1 + tanh u)^2 = cosh^2 u / e^{2u}. Also, sech^2 u = 1 / cosh^2 u. So putting it all together:

- tanh u / u * [ cosh^2 u / e^{2u} ] * [ 1 / cosh^2 u ] du = - tanh u / u * 1 / e^{2u} du. Simplify tanh u = sinh u / cosh u, so:

- (sinh u / cosh u) / u * e^{-2u} du = - sinh u / (u cosh u) * e^{-2u} du. Hmm, but sinh u = (e^u - e^{-u})/2, and cosh u = (e^u + e^{-u})/2. So sinh u / cosh u = (e^u - e^{-u})/(e^u + e^{-u}) = (e^{2u} -1)/(e^{2u} +1). So substituting back:

- [ (e^{2u} -1)/(e^{2u} +1) ] / u * e^{-2u} du. Let's multiply e^{-2u} into the numerator:

- [ (e^{2u} -1) e^{-2u} / (e^{2u} +1) ] / u du = - [ (1 - e^{-2u}) / (e^{2u} +1) ] / u du. Hmm, not sure if this is getting us anywhere. Maybe this substitution isn't helpful. Let me think of another approach.

Wait, going back to the original integral: ∫₀¹ (x -1)/[(x +1) ln x] dx. Let me consider substitution y = x. Wait, that's trivial. Alternatively, maybe expand the integrand as a series and integrate term by term. Let's see. The integrand is (x -1)/[(x +1) ln x]. Let me express (x -1)/(x +1) as a function and then expand 1/ln x as a series. But 1 x is near 0 and 1, so maybe expanding around x=1. Let me try to expand around x=1. Let t = 1 - x. Then as x approaches 1, t approaches 0. Let me see:

But maybe expanding (x -1)/ln x (x +1). Let me write x = 1 - t, so t = 1 - x. Then when x approaches 1, t approaches 0, and when x approaches 0, t approaches 1. Then dx = -dt. The integral becomes ∫₀¹ [ ( (1 - t) -1 ) / ( (1 - t) +1 ) ln(1 - t) ] (-dt). Simplify numerator: (1 - t -1) = -t. Denominator: (2 - t) ln(1 - t). So the integrand becomes (-t)/( (2 - t) ln(1 - t) ) * (-dt) = t/( (2 - t) ln(1 - t) ) dt. So the integral is ∫₀¹ t / [ (2 - t) ln(1 - t) ] dt. Hmm, not sure if that's better. Maybe expand ln(1 - t) as a series. ln(1 - t) = - Σ_{n=1}^∞ t^n /n for |t| <1. So 1/ln(1 - t) = -1 / Σ_{n=1}^∞ t^n /n. But that's a bit complicated. Alternatively, maybe write the integrand as t / [ (2 - t) (- Σ_{n=1}^∞ t^n /n ) ] = - t / [ (2 - t) Σ_{n=1}^∞ t^n /n ) ].

But this seems messy. Maybe another approach. Let me recall that sometimes integrals involving (x -1)/ln x can be related to the exponential integral or similar functions. Alternatively, perhaps differentiating under the integral sign. Let me consider introducing a parameter. Let me define I(a) = ∫₀¹ (x^a -1)/[(x +1) ln x] dx. Then, if we can compute I(a) and set a=1, that might work. Let's see. The idea is that differentiating the numerator x^a -1 with respect to a gives x^a ln x, which could cancel the denominator. Let's compute dI/da:

dI/da = ∫₀¹ [d/da (x^a -1)] / [ (x +1) ln x ] dx = ∫₀¹ [x^a ln x] / [ (x +1) ln x ] dx = ∫₀¹ x^a / (x +1) dx. So dI/da = ∫₀¹ x^a / (x +1) dx. Then, if we can compute this integral, we can integrate over a to find I(a), and then set a=1.

So first, compute ∫₀¹ x^a / (x +1) dx. Let's make substitution t = x +1, but maybe not helpful. Alternatively, write x^a / (x +1) as x^a * [1/(x +1)]. Alternatively, note that 1/(x +1) = ∫₀^∞ e^{-(x +1)t} dt. Then, interchange the order of integration. Let me try that.

So, ∫₀¹ x^a / (x +1) dx = ∫₀¹ x^a [ ∫₀^∞ e^{-(x +1)t} dt ] dx = ∫₀^∞ e^{-t} [ ∫₀¹ x^a e^{-xt} dx ] dt. Let's compute the inner integral ∫₀¹ x^a e^{-xt} dx. Let me make substitution u = xt, so x = u/t, dx = du/t. Then when x=0, u=0; x=1, u=t. So the integral becomes ∫₀^t ( (u/t)^a ) e^{-u} (du/t) ) = t^{-a -1} ∫₀^t u^a e^{-u} du. Therefore, the original integral becomes ∫₀^∞ e^{-t} [ t^{-a -1} ∫₀^t u^a e^{-u} du ] dt. Hmm, this seems complicated. Maybe another approach.

Alternatively, consider expanding 1/(x +1) as a series. For 0 ≤ x ≤1, 1/(x +1) = Σ_{n=0}^∞ (-1)^n x^n, which converges for |x| <1. But at x=1, it's an alternating series. So maybe integrating term by term. So ∫₀¹ x^a / (x +1) dx = ∫₀¹ x^a Σ_{n=0}^∞ (-1)^n x^n dx = Σ_{n=0}^∞ (-1)^n ∫₀¹ x^{a +n} dx = Σ_{n=0}^∞ (-1)^n / (a +n +1). So this is an infinite series. Therefore, dI/da = Σ_{n=0}^∞ (-1)^n / (a +n +1). Then, integrating this with respect to a from 0 to1 to get I(1) - I(0). Wait, but I(a) is defined as the integral from 0 to1 of (x^a -1)/[(x +1) ln x] dx. When a=0, the integrand becomes (1 -1)/[...] =0, so I(0)=0. Therefore, I(1) = ∫₀¹ dI/da da = ∫₀¹ Σ_{n=0}^∞ (-1)^n / (a +n +1) da. 

Integrate term by term: Σ_{n=0}^∞ (-1)^n ∫₀¹ 1/(a +n +1) da = Σ_{n=0}^∞ (-1)^n [ ln(a +n +1) ] from 0 to1 = Σ_{n=0}^∞ (-1)^n [ ln(n +2) - ln(n +1) ].

So I(1) = Σ_{n=0}^∞ (-1)^n [ ln(n +2) - ln(n +1) ] = Σ_{n=0}^∞ (-1)^n ln( (n +2)/(n +1) ). Let's see if this series can be summed. Let's write out the first few:

For n=0: (-1)^0 ln(2/1) = ln 2

n=1: (-1)^1 ln(3/2) = -ln(3/2)

n=2: (-1)^2 ln(4/3) = ln(4/3)

n=3: (-1)^3 ln(5/4) = -ln(5/4)

So the series is ln 2 - ln(3/2) + ln(4/3) - ln(5/4) + ... 

This telescopes in some way? Let's see:

Grouping terms:

ln 2 - ln(3/2) = ln 2 - (ln3 - ln2) = 2 ln2 - ln3

Then + ln(4/3) = 2 ln2 - ln3 + ln4 - ln3 = 2 ln2 + ln4 - 2 ln3

Wait, maybe not. Alternatively, write each term as ln[(n+2)/(n+1)]^((-1)^n). But the signs alternate. Let's write the series as Σ_{n=0}^∞ (-1)^n ln(1 + 1/(n+1)). Hmm, not sure. Alternatively, consider the product representation. The sum of logs is the log of the product. So:

Σ_{n=0}^∞ (-1)^n ln( (n+2)/(n+1) ) = ln [ Π_{n=0}^∞ ( (n+2)/(n+1) )^{ (-1)^n } ]

Let me write the product as:

For n even: (n+2)/(n+1) raised to 1

For n odd: (n+2)/(n+1) raised to -1

So the product becomes:

Π_{k=0}^∞ [ (2k +2)/(2k +1) ) * (2k +2)/(2k +3) )^{-1} ]

Wait, for n even: n=0,2,4,... So when n is even, say n=2k, term is (2k +2)/(2k +1). When n is odd, n=2k+1, term is (2k +3)/(2k +2), but raised to -1, so becomes (2k +2)/(2k +3). So the product becomes:

Π_{k=0}^∞ [ (2k +2)/(2k +1) * (2k +2)/(2k +3) ) ] = Π_{k=0}^∞ [ ( (2k +2)^2 ) / ( (2k +1)(2k +3) ) ) ]

This product resembles the Wallis product for π/2. The Wallis product is π/2 = Π_{k=1}^∞ [ (2k)^2 / ( (2k -1)(2k +1) ) ). But here, our product starts at k=0:

Π_{k=0}^∞ [ (2k +2)^2 / ( (2k +1)(2k +3) ) ) ] = Π_{k=0}^∞ [ (2(k+1))^2 / ( (2k +1)(2k +3) ) ) ] = Π_{k=1}^∞ [ (2k)^2 / ( (2k -1)(2k +1) ) ) ] * [ (2*0 +2)^2 / ( (2*0 +1)(2*0 +3) ) ) ] / [ (2*1)^2 / ( (2*1 -1)(2*1 +1) ) ) ]^{adjustment} Wait, maybe not. Let's see:

If we shift index m = k +1, then when k=0, m=1. So the product becomes:

For m=1 to ∞: (2m)^2 / ( (2m -1)(2m +1) ) ). But the original Wallis product is π/2 = Π_{m=1}^∞ [ (2m)^2 / ( (2m -1)(2m +1) ) ). So our product is exactly the Wallis product, which equals π/2. However, in our case, the product from k=0 to ∞ is the same as the Wallis product from m=1 to ∞ multiplied by the term at k=0. Let's check:

Original product: k=0 term is (2*0 +2)^2 / ( (2*0 +1)(2*0 +3) ) = (2)^2 / (1*3) = 4/3. Then for k=1, it's (4)^2/(3*5) = 16/15, etc. So the entire product is (4/3) * (16/15) * (36/35) * ... which is the same as the Wallis product starting from m=1, but multiplied by 4/3. Wait, the standard Wallis product starts with m=1: (2*1)^2/( (2*1 -1)(2*1 +1) ) = 4/(1*3) = 4/3, then next term is (4)^2/(3*5) = 16/15, etc. So actually, the product from k=0 to ∞ of [ (2k +2)^2 / ( (2k +1)(2k +3) ) ] is the same as the Wallis product from m=1 to ∞, which is π/2. Wait, but the standard Wallis product is π/2 = Π_{m=1}^∞ [ (4m^2)/(4m^2 -1) ) ] = Π_{m=1}^∞ [ (2m)^2 / ( (2m -1)(2m +1) ) ). So our product from k=0 to ∞ is exactly the same as the Wallis product from m=1 to ∞, which is π/2. Wait, but when k=0, the term is 4/3, which is the first term of the Wallis product. So the product from k=0 to ∞ is indeed the same as the Wallis product from m=1 to ∞, which equals π/2. Therefore, the product Π_{k=0}^∞ [ (2k +2)^2 / ( (2k +1)(2k +3) ) ] = π/2. Therefore, the original sum Σ_{n=0}^∞ (-1)^n ln( (n+2)/(n+1) ) = ln(π/2). Therefore, I(1) = ln(π/2). 

Therefore, the original integral ∫₀¹ (x -1)/[(x +1) ln x] dx = ln(π/2). 

Now, let's verify this result numerically. The exact answer is ln(π/2). Let's compute this numerically. π is approximately 3.1415926536, so π/2 ≈ 1.5707963268. The natural logarithm of that is ln(1.5707963268). Let's compute that. 

We know that ln(1) = 0, ln(e) ≈ 1.718..., but e is about 2.718. So 1.5708 is between 1/2 and e^{0.45} maybe. Let's compute it more accurately. Using a calculator, ln(1.5707963268) ≈ 0.4515827053. Let me check with a calculator. Yes, ln(π/2) ≈ 0.451582705289. Rounded to 10 decimal places, that's 0.4515827053.

So the exact answer is ln(π/2), and the numerical approximation is approximately 0.4515827053.
</think>

{"answer": "\\ln\\left(\\frac{\\pi}{2}\\right)", "numerical_answer": "0.4515827053"}