To evaluate the definite integral

$$
\int_0^{\frac{\pi}{4}} \tan^{-1}\left(\frac{1+\tan(x)}{\sqrt{2}}\right)\,dx,
$$

we proceed using a clever substitution and properties of the inverse tangent function.

---

### Step 1: Use Substitution

Let us perform the substitution:

$$
x = \frac{\pi}{4} - t \quad \Rightarrow \quad dx = -dt.
$$

When $ x = 0 $, $ t = \frac{\pi}{4} $, and when $ x = \frac{\pi}{4} $, $ t = 0 $. The integral becomes:

$$
\int_0^{\frac{\pi}{4}} \tan^{-1}\left(\frac{1+\tan(x)}{\sqrt{2}}\right)\,dx = \int_{\frac{\pi}{4}}^{0} \tan^{-1}\left(\frac{1+\tan\left(\frac{\pi}{4} - t\right)}{\sqrt{2}}\right)(-dt).
$$

This simplifies to:

$$
\int_0^{\frac{\pi}{4}} \tan^{-1}\left(\frac{1+\tan\left(\frac{\pi}{4} - t\right)}{\sqrt{2}}\right)\,dt.
$$

---

### Step 2: Simplify the Expression

Recall the identity:

$$
\tan\left(\frac{\pi}{4} - t\right) = \frac{1 - \tan t}{1 + \tan t}.
$$

Substitute this into the integrand:

$$
\frac{1 + \tan\left(\frac{\pi}{4} - t\right)}{\sqrt{2}} = \frac{1 + \frac{1 - \tan t}{1 + \tan t}}{\sqrt{2}} = \frac{(1 + \tan t) + (1 - \tan t)}{(1 + \tan t)\sqrt{2}} = \frac{2}{(1 + \tan t)\sqrt{2}} = \frac{\sqrt{2}}{1 + \tan t}.
$$

Thus, the transformed integrand becomes:

$$
\tan^{-1}\left(\frac{\sqrt{2}}{1 + \tan t}\right).
$$

So the original integral becomes:

$$
\int_0^{\frac{\pi}{4}} \tan^{-1}\left(\frac{1 + \tan x}{\sqrt{2}}\right)\,dx = \int_0^{\frac{\pi}{4}} \tan^{-1}\left(\frac{\sqrt{2}}{1 + \tan x}\right)\,dx.
$$

---

### Step 3: Add the Two Forms

Let the original integral be $ I $. Then:

$$
I = \int_0^{\frac{\pi}{4}} \tan^{-1}\left(\frac{1 + \tan x}{\sqrt{2}}\right)\,dx = \int_0^{\frac{\pi}{4}} \tan^{-1}\left(\frac{\sqrt{2}}{1 + \tan x}\right)\,dx.
$$

Now, consider the sum:

$$
2I = \int_0^{\frac{\pi}{4}} \left[ \tan^{-1}\left(\frac{1 + \tan x}{\sqrt{2}}\right) + \tan^{-1}\left(\frac{\sqrt{2}}{1 + \tan x}\right) \right] dx.
$$

Let $ A = \frac{1 + \tan x}{\sqrt{2}} $, then the second term is $ \tan^{-1}(1/A) $. Since $ A > 0 $ for all $ x \in [0, \frac{\pi}{4}] $, we apply the identity:

$$
\tan^{-1}(A) + \tan^{-1}(1/A) = \frac{\pi}{2}.
$$

Therefore, the integrand becomes $ \frac{\pi}{2} $, and the integral simplifies to:

$$
2I = \int_0^{\frac{\pi}{4}} \frac{\pi}{2} \, dx = \frac{\pi}{2} \cdot \frac{\pi}{4} = \frac{\pi^2}{8}.
$$

Dividing both sides by 2:

$$
I = \frac{\pi^2}{16}.
$$

---

### Step 4: Numerical Approximation

$$
\frac{\pi^2}{16} \approx \frac{(3.