Let's solve the integral:
\[
I = \int_{0}^{1} \arcsin\left(0.5\sqrt{x(1-x)}\right) dx
\]

**Step 1: Symmetry and substitution**

Let \( x = \sin^2 \theta \), so \( dx = 2 \sin\theta \cos\theta d\theta = \sin 2\theta d\theta \).  
When \( x = 0 \rightarrow \theta = 0 \);  
when \( x = 1 \rightarrow \theta = \frac{\pi}{2} \).

Also,
\[
x(1-x) = \sin^2\theta (1 - \sin^2\theta) = \sin^2\theta\cos^2\theta = \frac{1}{4}\sin^2 2\theta
\]
So,
\[
0.5\sqrt{x(1-x)} = 0.5 \cdot \frac{1}{2}|\sin 2\theta| = \frac{1}{4}|\sin 2\theta|
\]
But for \( \theta \) from \( 0 \) to \( \pi/2 \), \( \sin 2\theta \geq 0 \), so it is just \( \frac{1}{4}\sin 2\theta \).

Therefore,
\[
I = \int_{x=0}^{x=1} \arcsin\left(0.5\sqrt{x(1-x)}\right)dx
= \int_{\theta=0}^{\theta=\frac{\pi}{2}} \arcsin\left(\frac{1}{4}\sin 2\theta\right) \sin 2\theta d\theta
\]

**Step 2: Simplify the integral**

Let us now write:
\[
I = \int_{0}^{\frac{\pi}{2}} \arcsin\left(\frac{1}{4}\sin 2\theta\right) \sin 2\theta d\theta
\]

Let \( u = 2\theta \Rightarrow \theta = \frac{u}{2}, d\theta = \frac{du}{2} \).  
As \( \theta \) goes from \( 0 \) to \( \frac{\pi}{2} \), \( u \) goes from \( 0 \) to \( \pi \).

\[
I = \int_{u=0}^{u=\pi} \arcsin\left(\frac{1}{4}\sin u\right) \sin u \cdot \frac{du}{2}
= \frac{1}{2}\int_{0}^{\pi} \arcsin\left(\frac{1}{4}\sin u\right)\sin u du
\]

Let us denote:
\[
J = \int_{0}^{\pi} \arcsin\left(\frac{1}{4}\sin u\right)\sin u du,
\]
so \( I = \frac{J}{2} \).

**Step 3: Compute \( J \) by parts**

Let’s perform integration by parts:
Let \( f(u) = \arcsin\left(\frac{1}{4}\sin u\right) \), \( dg = \sin u du \),
then \( df = \frac{1}{\sqrt{1 - (\frac{1}{4}\sin u)^2}}\cdot \frac{1}{4}\cos u du = \frac{\cos u}{4\sqrt{1 - \frac{1}{16}\sin^2 u}} du \),
and \( g = -\cos u \).

So,
\[
J = \left. -\arcsin\left(\frac{1}{4}\sin u\right)\cos u \right|_0^{\pi} + \int_{0}^{\pi} \cos u \cdot \frac{1}{\sqrt{1 - (\frac{1}{4}\sin u)^2}} \cdot \frac{1}{4} \cos u du
\]

But at \( u = 0, \sin u = 0, \cos u = 1 \) and \( u = \pi, \sin u = 0, \cos u = -1 \), and \( \arcsin(0) = 0 \), so the first term is:
\[
-\arcsin(0)\cdot\cos(\pi) + \arcsin(0)\cdot\cos(0) = 0
\]

So,
\[
J = \frac{1}{4} \int_{0}^{\pi} \frac{\cos^2 u}{\sqrt{1 - \frac{1}{16}\sin^2 u}} du
\]

Thus,
\[
I = \frac{J}{2} = \frac{1}{8} \int_{0}^{\pi} \frac{\cos^2 u}{\sqrt{1 - \frac{1}{16}\sin^2 u}} du
\]

**Step 4: Express \(\cos^2 u\) in terms of \(\cos 2u\)**

Recall, \( \cos^2 u = \frac{1+\cos 2u}{2} \):

\[
I = \frac{1}{8}\int_0^\pi \frac{1+\cos 2u}{2\sqrt{1-\frac{1}{16}\sin^2 u}} du
= \frac{1}{16}\int_0^\pi \frac{du}{\sqrt{1-\frac{1}{16}\sin^2 u}}
+ \frac{1}{16} \int_0^\pi \frac{\cos 2u \, du}{\sqrt{1-\frac{1}{16}\sin^2 u}}
\]

But the second term vanishes because the integrand is an odd function about \( u = \pi/2 \) over \( [0,\pi] \):
Let’s check: \( \sin^2(\pi-u) = \sin^2 u \), \( \cos 2(\pi-u) = \cos(2\pi-2u)=\cos 2u \), so it's actually an even function, but \(\cos 2u\) averages to zero over a period. But let's numerically or formally note that usually the average of \(\cos 2u\) over \(0\) to \(\pi\) is zero when multiplied by even function.

Let's check this assertion. Let’s try to compute further.

Let
\[
K = \int_{0}^{\pi} \frac{\cos 2u}{\sqrt{1-\frac{1}{16}\sin^2 u}} du
\]
Let \( v = \pi - u \), \( du = -dv \), so as \( u: 0 \rightarrow \pi \), \( v: \pi \rightarrow 0 \):

\[
K = \int_{v=\pi}^{v=0} \frac{\cos 2(\pi - v)}{\sqrt{1-\frac{1}{16}\sin^2(\pi-v)}} (-dv) = \int_{v=0}^{v=\pi} \frac{\cos (2v)}{\sqrt{1-\frac{1}{16}\sin^2 v}} dv
\]

So the integral is actually symmetric and not zero. So the term remains.

**Step 5: Express in terms of elliptic integrals**

Recall, the standard complete elliptic integral of the first and second kind:

\[
K(k) = \int_{0}^{\frac{\pi}{2}} \frac{d\theta}{\sqrt{1-k^2 \sin^2 \theta}}, \quad
E(k) = \int_{0}^{\frac{\pi}{2}} \sqrt{1 - k^2 \sin^2 \theta} d\theta
\]

Our integral:
\[
\int_0^\pi \frac{du}{\sqrt{1 - \frac{1}{16}\sin^2 u}} = 2 \int_0^{\frac{\pi}{2}} \frac{du}{\sqrt{1 - \frac{1}{16}\sin^2 u}} = 2K\left(\frac{1}{4}\right)
\]

Similarly:

Let’s now try to express \( \int_0^\pi \frac{\cos 2u}{\sqrt{1-\frac{1}{16}\sin^2 u}} du \).

Recall:

\[
\int_0^\pi \frac{\cos 2u}{\sqrt{1 - k^2 \sin^2 u}} du = 2 \int_0^{\frac{\pi}{2}} \frac{\cos 2u}{\sqrt{1 - k^2 \sin^2 u}} du
\]

But,
\[
\cos 2u = 1 - 2 \sin^2 u
\]
Therefore,
\[
\int_0^\pi \frac{\cos 2u}{\sqrt{1 - k^2 \sin^2 u}} du
= \int_0^\pi \frac{du}{\sqrt{1-k^2 \sin^2 u}} - 2 \int_0^\pi \frac{\sin^2 u}{\sqrt{1-k^2 \sin^2 u}} du
\]
But the first term we just computed; for the second, recall:

\[
\int_0^\pi \frac{\sin^2 u}{\sqrt{1-k^2 \sin^2 u}} du = 2 \int_0^{\frac{\pi}{2}} \frac{\sin^2 u}{\sqrt{1 - k^2 \sin^2 u}} du
\]

Now,
\[
\int_0^{\frac{\pi}{2}} \frac{\sin^2 u}{\sqrt{1 - k^2 \sin^2 u}} du = \frac{1}{k^2} \left( K(k) - E(k) \right)
\]
Therefore,
\[
\int_0^\pi \frac{\sin^2 u}{\sqrt{1 - k^2 \sin^2 u}} du = \frac{2}{k^2} \left(K(k) - E(k)\right)
\]

For \( k = \frac{1}{4} \):

So, our key terms are:

First term:
\[
A = \int_0^\pi \frac{du}{\sqrt{1-\frac{1}{16}\sin^2 u}} = 2K\left(\frac{1}{4}\right)
\]

Second term:
\[
B = \int_0^\pi \frac{\sin^2 u}{\sqrt{1-\frac{1}{16}\sin^2 u}} du = 2 \times \frac{K(\frac{1}{4}) - E(\frac{1}{4})}{(\frac{1}{4})^2} = 2 \times \frac{K(\frac{1}{4}) - E(\frac{1}{4})}{1/16} = 32\left(K(\frac{1}{4}) - E(\frac{1}{4})\right)
\]

Therefore,
\[
\int_0^\pi \frac{\cos 2u}{\sqrt{1-\frac{1}{16}\sin^2 u}} du = A - 2B = 2K\left(\frac{1}{4}\right) - 64 \left(K(\frac{1}{4}) - E(\frac{1}{4})\right) = 2K\left(\frac{1}{4}\right) - 64 K(\frac{1}{4}) + 64 E(\frac{1}{4}) = (2 - 64)K\left(\frac{1}{4}\right) + 64 E\left(\frac{1}{4}\right) = -62 K\left(\frac{1}{4}\right) + 64 E\left(\frac{1}{4}\right)
\]

Back to our expression for \( I \):

\[
I = \frac{1}{16} \left[ 2 K\left(\frac{1}{4}\right) + \left(-62 K\left(\frac{1}{4}\right) + 64 E\left(\frac{1}{4}\right)\right) \right]
= \frac{1}{16} \left[ -60 K\left(\frac{1}{4}\right) + 64 E\left(\frac{1}{4}\right) \right]
= \frac{1}{16} \left( 64 E\left(\frac{1}{4}\right) - 60 K\left(\frac{1}{4}\right) \right)
= 4 E\left(\frac{1}{4}\right) - \frac{15}{4} K\left(\frac{1}{4}\right)
\]

**Step 6: Final Answer**

So,

\[
\boxed{
I = 4 E\left(\frac{1}{4}\right) - \frac{15}{4} K\left(\frac{1}{4}\right)
}
\]

Where \( K \) and \( E \) are the complete elliptic integrals of the first and second kind.

**Step 7: Numerical evaluation**

Let’s numerically evaluate:

- \( K(1/4) \approx 1.5743520850 \)
- \( E(1/4) \approx 1.4674622093 \)

So,

\[
I \approx 4 \times 1.4674622093 - \frac{15}{4} \times 1.5743520850
\]
\[
= 5.8698488372 - 5.9045703188
= -0.0347214816
\]

Rounded to 10 decimal places: \(\boxed{-0.0347214816}\)

**Step 8: Output in JSON**

```json
{"answer": "4 E\\left(\\frac{1}{4}\\right) - \\frac{15}{4} K\\left(\\frac{1}{4}\\right)", "numerical_answer": "-0.0347214816"}
```