
To solve the definite integral \(\int\limits_0^{2} x^{-1/2} \left[1 + \sqrt{x(2 - x)}\right]^{-3/2} \, dx\), we proceed with the following steps:

### Step 1: Trigonometric Substitution
Let \( x = 2 \sin^2 \theta \). This substitution simplifies the square root term \( \sqrt{x(2 - x)} \):
- \( dx = 4 \sin\theta \cos\theta \, d\theta \)
- When \( x = 0 \), \( \theta = 0 \); when \( x = 2 \), \( \theta = \frac{\pi}{2} \).
- \( \sqrt{x(2 - x)} = \sqrt{2 \sin^2 \theta \cdot 2 \cos^2 \theta} = 2 \sin\theta \cos\theta \).

### Step 2: Simplify the Integrand
Substituting \( x = 2 \sin^2 \theta \) into the integrand:
- \( x^{-1/2} = (2 \sin^2 \theta)^{-1/2} = \frac{1}{\sqrt{2} \sin\theta} \)
- \( 1 + \sqrt{x(2 - x)} = 1 + 2 \sin\theta \cos\theta = (\sin\theta + \cos\theta)^2 \) (using the identity \( (\sin\theta + \cos\theta)^2 = 1 + 2 \sin\theta \cos\theta \))
- Thus, \( \left[1 + \sqrt{x(2 - x)}\right]^{-3/2} = (\sin\theta + \cos\theta)^{-3} \).

The integrand becomes:
\[
x^{-1/2} \left[1 + \sqrt{x(2 - x)}\right]^{-3/2} dx = \frac{1}{\sqrt{2} \sin\theta} \cdot (\sin\theta + \cos\theta)^{-3} \cdot 4 \sin\theta \cos\theta \, d\theta
\]
Simplifying, the \( \sin\theta \) terms cancel, leaving:
\[
\frac{4}{\sqrt{2}} \cos\theta (\sin\theta + \cos\theta)^{-3} d\theta = 2\sqrt{2} \cos\theta (\sin\theta + \cos\theta)^{-3} d\theta
\]

### Step 3: Substitution \( t = \tan\theta \)
Let \( t = \tan\theta \), so \( \theta = \arctan t \), \( d\theta = \frac{dt}{1 + t^2} \), \( \sin\theta = \frac{t}{\sqrt{1 + t^2}} \), and \( \cos\theta = \frac{1}{\sqrt{1 + t^2}} \). Then:
- \( \sin\theta + \cos\theta = \frac{t + 1}{\sqrt{1 + t^2}} \)
- \( (\sin\theta + \cos\theta)^{-3} = \frac{(1 + t^2)^{3/2}}{(t + 1)^3} \)
- \( \cos\theta \, d\theta = \frac{1}{\sqrt{1 + t^2}} \cdot \frac{dt}{1 + t^2} = \frac{dt}{(1 + t^2)^{3/2}} \).

Substituting these into the integrand:
\[
2\sqrt{2} \cdot \frac{dt}{(1 + t^2)^{3/2}} \cdot \frac{(1 + t^2)^{3/2}}{(t + 1)^3} = 2\sqrt{2} \cdot \frac{dt}{(t + 1)^3}
\]

### Step 4: Evaluate the Integral
The integral now simplifies to:
\[
2\sqrt{2} \int_{0}^{\infty} \frac{dt}{(t + 1)^3}
\]
The antiderivative of \( (t + 1)^{-3} \) is \( -\frac{1}{2(t + 1)^2} \). Evaluating from \( 0 \) to \( \infty \):
\[
2\sqrt{2} \left[ \lim_{t \to \infty} \left( -\frac{1}{2(t + 1)^2} \right) - \left( -\frac{1}{2(0 + 1)^2} \right) \right] = 2\sqrt{2} \left( 0 + \frac{1}{2} \right) = \sqrt{2}
\]

### Numerical Approximation
The exact value is \( \sqrt{2} \approx 1.4142135624 \) (rounded to 10 decimal places).

{"answer": "\(\sqrt{2}\)", "numerical_answer": "1.4142135624"}