To solve the definite integral \(\int_0^\infty \frac{\sin \sqrt{3} x - \sin \frac{x}{\sqrt{3}}}{x} e^{-x^2} \, dx\), we will follow the steps outlined.

### Step 1: Analytical Computation

First, let's rewrite the integral for clarity:
\[ I = \int_0^\infty \frac{\sin \sqrt{3} x - \sin \frac{x}{\sqrt{3}}}{x} e^{-x^2} \, dx. \]

We can split this into two separate integrals:
\[ I = \int_0^\infty \frac{\sin \sqrt{3} x}{x} e^{-x^2} \, dx - \int_0^\infty \frac{\sin \frac{x}{\sqrt{3}}}{x} e^{-x^2} \, dx. \]

Let's denote these integrals as \(I_1\) and \(I_2\):
\[ I_1 = \int_0^\infty \frac{\sin \sqrt{3} x}{x} e^{-x^2} \, dx, \]
\[ I_2 = \int_0^\infty \frac{\sin \frac{x}{\sqrt{3}}}{x} e^{-x^2} \, dx. \]

### Step 2: Evaluate \(I_1\)

Consider the integral \(I_1\):
\[ I_1 = \int_0^\infty \frac{\sin \sqrt{3} x}{x} e^{-x^2} \, dx. \]

We use the substitution \(u = \sqrt{3} x\), so \(du = \sqrt{3} dx\) and \(dx = \frac{du}{\sqrt{3}}\):
\[ I_1 = \int_0^\infty \frac{\sin u}{\frac{u}{\sqrt{3}}} e^{-\left(\frac{u}{\sqrt{3}}\right)^2} \frac{du}{\sqrt{3}} = \int_0^\infty \frac{\sin u}{u} e^{-\frac{u^2}{3}} \, du. \]

This integral is a known result involving the sine integral function \(\text{Si}(x)\) and the Gaussian integral:
\[ \int_0^\infty \frac{\sin u}{u} e^{-a u^2} \, du = \frac{\pi}{2} \text{erf}\left(\frac{1}{2\sqrt{a}}\right), \]
where \(\text{erf}(x)\) is the error function.

For \(a = \frac{1}{3}\):
\[ I_1 = \frac{\pi}{2} \text{erf}\left(\frac{\sqrt{3}}{2}\right). \]

### Step 3: Evaluate \(I_2\)

Consider the integral \(I_2\):
\[ I_2 = \int_0^\infty \frac{\sin \frac{x}{\sqrt{3}}}{x} e^{-x^2} \, dx. \]

We use the substitution \(v = \frac{x}{\sqrt{3}}\), so \(dv = \frac{dx}{\sqrt{3}}\) and \(dx = \sqrt{3} dv\):
\[ I_2 = \int_0^\infty \frac{\sin v}{\frac{v}{\sqrt{3}}} e^{-3 v^2} \sqrt{3} \, dv = \int_0^\infty \frac{\sin v}{v} e^{-3 v^2} \, dv. \]

Using the same known result:
\[ \int_0^\infty \frac{\sin v}{v} e^{-b v^2} \, dv = \frac{\pi}{2} \text{erf}\left(\frac{1}{2\sqrt{b}}\right), \]
where \(b = 3\):
\[ I_2 = \frac{\pi}{2} \text{erf}\left(\frac{1}{2\sqrt{3}}\right). \]

### Step 4: Combine the Results

Combining \(I_1\) and \(I_2\):
\[ I = I_1 - I_2 = \frac{\pi}{2} \text{erf}\left(\frac{\sqrt{3}}{2}\right) - \frac{\pi}{2} \text{erf}\left(\frac{1}{2\sqrt{3}}\right). \]

### Step 5: Numerical Approximation

Using numerical values for the error functions:
\[ \text{erf}\left(\frac{\sqrt{3}}{2}\right) \approx 0.9973, \]
\[ \text{erf}\left(\frac{1}{2\sqrt{3}}\right) \approx 0.3173. \]

Thus:
\[ I \approx \frac{\pi}{2} (0.9973 - 0.3173) = \frac{\pi}{2} \times 0.68 = 1.0681415022. \]

### Final Answer

The exact answer in LaTeX format and the numerical approximation rounded to 10 decimal places are:
```json
{"answer": "\\frac{\\pi}{2} \\left( \\text{erf}\\left(\\frac{\\sqrt{3}}{2}\\right) - \\text{erf}\\left(\\frac{1}{2\\sqrt{3}}\\right) \\right)", "numerical_answer": "1.0681415022"}
```