# Calculating the definite integral $\int_{\frac18}^{\frac14}\frac{\ln(2x)\ln(4x)\ln(8x)}x\:\mathrm{d}x$

## Step 1: Simplify the integrand

Let's first simplify the integrand by rewriting $\ln(2x)$, $\ln(4x)$, and $\ln(8x)$ in terms of $\ln(x)$ and constants.

$\ln(2x) = \ln(2) + \ln(x)$
$\ln(4x) = \ln(4) + \ln(x) = \ln(2^2) + \ln(x) = 2\ln(2) + \ln(x)$
$\ln(8x) = \ln(8) + \ln(x) = \ln(2^3) + \ln(x) = 3\ln(2) + \ln(x)$

Now, let's expand the product:
$\ln(2x)\ln(4x)\ln(8x) = [\ln(2) + \ln(x)][2\ln(2) + \ln(x)][3\ln(2) + \ln(x)]$

Multiplying these terms:
$= [\ln(2) + \ln(x)][6\ln(2)\ln(2) + 3\ln(2)\ln(x) + 2\ln(2)\ln(x) + \ln(x)\ln(x)]$
$= [\ln(2) + \ln(x)][6\ln^2(2) + 5\ln(2)\ln(x) + \ln^2(x)]$

Expanding further:
$= \ln(2)[6\ln^2(2) + 5\ln(2)\ln(x) + \ln^2(x)] + \ln(x)[6\ln^2(2) + 5\ln(2)\ln(x) + \ln^2(x)]$
$= 6\ln^3(2) + 5\ln^2(2)\ln(x) + \ln(2)\ln^2(x) + 6\ln(2)^2\ln(x) + 5\ln(2)\ln^2(x) + \ln^3(x)$
$= 6\ln^3(2) + 11\ln^2(2)\ln(x) + 6\ln(2)\ln^2(x) + \ln^3(x)$

## Step 2: Set up the integral with the expanded integrand

Our integral becomes:
$\int_{\frac18}^{\frac14}\frac{6\ln^3(2) + 11\ln^2(2)\ln(x) + 6\ln(2)\ln^2(x) + \ln^3(x)}{x}\:\mathrm{d}x$

Let's split this into separate integrals:
$\int_{\frac18}^{\frac14}\frac{6\ln^3(2)}{x}\:\mathrm{d}x + \int_{\frac18}^{\frac14}\frac{11\ln^2(2)\ln(x)}{x}\:\mathrm{d}x + \int_{\frac18}^{\frac14}\frac{6\ln(2)\ln^2(x)}{x}\:\mathrm{d}x + \int_{\frac18}^{\frac14}\frac{\ln^3(x)}{x}\:\mathrm{d}x$

## Step 3: Evaluate each integral

### For $\int_{\frac18}^{\frac14}\frac{6\ln^3(2)}{x}\:\mathrm{d}x$:
This is $6\ln^3(2) \int_{\frac18}^{\frac14}\frac{1}{x}\:\mathrm{d}x = 6\ln^3(2)[\ln(x)]_{\frac18}^{\frac14} = 6\ln^3(2)[\ln(\frac14) - \ln(\frac18)] = 6\ln^3(2)[\ln(2)]$
$= 6\ln^4(2)$

### For $\int_{\frac18}^{\frac14}\frac{11\ln^2(2)\ln(x)}{x}\:\mathrm{d}x$:
Using the formula $\int \frac{\ln^n(x)}{x}dx = \frac{\ln^{n+1}(x)}{n+1} + C$:
$11\ln^2(2) \int_{\frac18}^{\frac14}\frac{\ln(x)}{x}\:\mathrm{d}x = 11\ln^2(2)[\frac{\ln^2(x)}{2}]_{\frac18}^{\frac14}$
$= \frac{11\ln^2(2)}{2}[\ln^2(\frac14) - \ln^2(\frac18)]$
$= \frac{11\ln^2(2)}{2}[(-2\ln(2))^2 - (-3\ln(2))^2]$
$= \frac{11\ln^2(2)}{2}[4\ln^2(2) - 9\ln^2(2)]$
$= \frac{11\ln^2(2)}{2}[-5\ln^2(2)]$
$= -\frac{55\ln^4(2)}{2}$

### For $\int_{\frac18}^{\frac14}\frac{6\ln(2)\ln^2(x)}{x}\:\mathrm{d}x$:
$6\ln(2) \int_{\frac18}^{\frac14}\frac{\ln^2(x)}{x}\:\mathrm{d}x = 6\ln(2)[\frac{\ln^3(x)}{3}]_{\frac18}^{\frac14}$
$= 2\ln(2)[\ln^3(\frac14) - \ln^3(\frac18)]$
$= 2\ln(2)[(-2\ln(2))^3 - (-3\ln(2))^3]$
$= 2\ln(2)[-8\ln^3(2) - (-27\ln^3(2))]$
$= 2\ln(2)[19\ln^3(2)]$
$= 38\ln^4(2)$

### For $\int_{\frac18}^{\frac14}\frac{\ln^3(x)}{x}\:\mathrm{d}x$:
$\int_{\frac18}^{\frac14}\frac{\ln^3(x)}{x}\:\mathrm{d}x = [\frac{\ln^4(x)}{4}]_{\frac18}^{\frac14}$
$= \frac{1}{4}[\ln^4(\frac14) - \ln^4(\frac18)]$
$= \frac{1}{4}[(-2\ln(2))^4 - (-3\ln(2))^4]$
$= \frac{1}{4}[16\ln^4(2) - 81\ln^4(2)]$
$= \frac{1}{4}[-65\ln^4(2)]$
$= -\frac{65\ln^4(2)}{4}$

## Step 4: Combine all parts to get the final result

$\int_{\frac18}^{\frac14}\frac{\ln(2x)\ln(4x)\ln(8x)}{x}\:\mathrm{d}x = 6\ln^4(2) - \frac{55\ln^4(2)}{2} + 38\ln^4(2) - \frac{65\ln^4(2)}{4}$
$= \ln^4(2)(6 - \frac{55}{2} + 38 - \frac{65}{4})$
$= \ln^4(2)(6 - \frac{110}{4} + 38 - \frac{65}{4})$
$= \ln^4(2)(6 - \frac{110}{4} + \frac{152}{4} - \frac{65}{4})$
$= \ln^4(2)(6 + \frac{-110 + 152 - 65}{4})$
$= \ln^4(2)(6 + \frac{-23}{4})$
$= \ln^4(2)(\frac{24 - 23}{4})$
$= \ln^4(2)(\frac{1}{4})$
$= \frac{\ln^4(2)}{4}$

## Step 5: Numerical approximation

$\ln(2) \approx 0.6931471806$
$\ln^4(2) \approx 0.2311914274$
$\frac{\ln^4(2)}{4} \approx 0.0577978568$

## Final result

The definite integral $\int_{\frac18}^{\frac14}\frac{\ln(2x)\ln(4x)\ln(8x)}{x}\:\mathrm{d}x = \frac{\ln^4(2)}{4}$

{"answer": "\\frac{\\ln^4(2)}{4}", "numerical_answer": "0.0577978568"}