We wish to evaluate

  I = ∫₀² x^(–1/2)[1 + √(x(2 – x))]^(–3/2) dx.

Step 1. Substitution x = 2 sin²θ

Let
  x = 2 sin²θ   →  dx = 4 sinθ cosθ dθ.
Then when x = 0, sinθ = 0 so θ = 0; and when x = 2, sin²θ = 1 so θ = π/2.

Also,
  x^(–1/2) = (2 sin²θ)^(–1/2) = 1/(√2 sinθ).
and
  √(x(2 – x)) = √(2 sin²θ·[2 – 2 sin²θ])
           = √(4 sin²θ cos²θ) = 2 sinθ cosθ   (since 0 ≤ θ ≤ π/2).

Thus the bracket becomes:
  [1 + √(x(2 – x))]^(–3/2) = [1 + 2 sinθ cosθ]^(–3/2).

Substitute everything into I:
  I = ∫₀^(π/2) [1/(√2 sinθ)] · [1 + 2 sinθ cosθ]^(–3/2) · [4 sinθ cosθ dθ]
    = (4 cosθ/(√2)) [1 + 2 sinθ cosθ]^(–3/2) dθ.
That is,
  I = 2√2 ∫₀^(π/2) cosθ [1 + 2 sinθ cosθ]^(–3/2) dθ.

Step 2. Write 2 sinθ cosθ = sin(2θ)

Then
  I = 2√2 ∫₀^(π/2) cosθ [1 + sin(2θ)]^(–3/2) dθ.

Step 3. Change variable to z = 2θ

Let z = 2θ, so dθ = dz/2; when θ = 0, z = 0; and when θ = π/2, z = π. Also, cosθ becomes cos(z/2). Then
  I = 2√2 ∫₀^(π) cos(z/2) [1 + sinz]^(–3/2) (dz/2)
    = √2 ∫₀^(π) cos(z/2) [1 + sinz]^(–3/2) dz.

Step 4. Write 1 + sinz as a square

Notice that
  (sin(z/2) + cos(z/2))² = sin²(z/2) + cos²(z/2) + 2 sin(z/2) cos(z/2)
          = 1 + sinz.
Thus,
  [1 + sinz]^(–3/2) = [ (sin(z/2) + cos(z/2))² ]^(–3/2) = [sin(z/2) + cos(z/2)]^(–3).

So
  I = √2 ∫₀^(π) cos(z/2) [sin(z/2) + cos(z/2)]^(–3) dz.

Step 5. Substitute u = z/2

Let u = z/2, hence z = 2u and dz = 2 du. When z goes from 0 to π, u goes from 0 to π/2. Then
  I = √2 ∫₀^(π/2) cos u [sin u + cos u]^(–3) · 2 du
    = 2√2 ∫₀^(π/2) cos u/(sin u + cos u)³ du.

Step 6. Substitute u = π/4 – w

Define w = (π/4) – u so that u = π/4 – w and du = –dw. When u = 0, w = π/4, and when u = π/2, w = –π/4. Express sin u and cos u in terms of w:
  sin u = sin(π/4 – w) = (1/√2)(cos w – sin w),
  cos u = cos(π/4 – w) = (1/√2)(cos w + sin w).
Then,
  sin u + cos u = (1/√2)[(cos w – sin w) + (cos w + sin w)] = (1/√2)(2 cos w) = √2 cos w.
Thus, (sin u + cos u)³ = (√2 cos w)³ = 2√2 cos³w.

Also, cos u = (1/√2)(cos w + sin w).

Now substitute into the u-integral (and change limits accordingly):
  I = 2√2 ∫_(u=0)^(π/2) cos u/(sin u + cos u)³ du
    = 2√2 ∫_(w=π/4)^(–π/4) [(1/√2)(cos w + sin w)]/(2√2 cos³w) (–dw).
Take the constants:
  2√2 · (1/√2) = 2,
and denominator constant 2√2 remains, so overall constant is 2/(2√2) = 1/√2. Reversing the limits yields:
  I = (1/√2) ∫_(w=–π/4)^(π/4) (cos w + sin w)/cos³w dw.

Step 7. Write integrand as a sum of two functions

Break the integrand:
  (cos w + sin w)/cos³w = cos w/cos³w + sin w/cos³w = 1/cos²w + (sin w)/(cos³w) = sec²w + tan w·sec²w.
Thus,
  I = (1/√2) [∫_(–π/4)^(π/4) sec²w dw + ∫_(–π/4)^(π/4) tan w sec²w dw].

Step 8. Evaluate the two integrals

We compute:
  ∫ sec²w dw = tan w.
and
  ∫ tan w sec²w dw.
Let u = tan w so that du = sec²w dw, and the integral becomes ∫ u du = (u²)/2 = (tan²w)/2.

Thus, the antiderivative is:
  F(w) = tan w + (tan²w)/2.
We now evaluate from w = –π/4 to w = π/4.

At w = π/4, tan(π/4) = 1, so F(π/4) = 1 + 1/2 = 3/2.
At w = –π/4, tan(–π/4) = –1, and tan²(–π/4) = 1, so F(–π/4) = (–1) + 1/2 = –1/2.
Thus the difference is:
  F(π/4) – F(–π/4) = (3/2) – (–1/2) = 2.

Then,
  I = (1/√2) · 2 = 2/√2 = √2.

Step 9. Conclusion and Numerical Approximation

The exact value of the integral is √2 and numerically
  √2 ≈ 1.4142135624 (to 10 decimal places).

The final answer in the required JSON format is:
{"answer": "\\sqrt{2}", "numerical_answer": "1.4142135624"}