

To calculate the definite integral \(\int_0^\pi \cos(x + \cos x) \, dx\), we proceed as follows:

### Step 1: Substitution to Simplify the Integral
Consider the substitution \(x = \pi - t\). When \(x = 0\), \(t = \pi\), and when \(x = \pi\), \(t = 0\). The differential \(dx = -dt\). Substituting into the integral:

\[
\int_0^\pi \cos(x + \cos x) \, dx = \int_\pi^0 \cos\left((\pi - t) + \cos(\pi - t)\right) (-dt)
\]

Simplify the argument of the cosine function. Since \(\cos(\pi - t) = -\cos t\), we have:

\[
(\pi - t) + \cos(\pi - t) = \pi - t - \cos t = \pi - (t + \cos t)
\]

Thus, the integral becomes:

\[
\int_0^\pi \cos\left(\pi - (t + \cos t)\right) \, dt
\]

### Step 2: Using a Trigonometric Identity
Recall that \(\cos(\pi - A) = -\cos A\). Applying this identity:

\[
\int_0^\pi \cos\left(\pi - (t + \cos t)\right) \, dt = \int_0^\pi -\cos(t + \cos t) \, dt
\]

### Step 3: Relating the Original Integral to Itself
Let \(I = \int_0^\pi \cos(x + \cos x) \, dx\). From the substitution above, we find:

\[
I = -\int_0^\pi \cos(t + \cos t) \, dt = -I
\]

This implies \(I = -I\), so \(2I = 0\), hence \(I = 0\).

### Numerical Approximation
The exact value of the integral is \(0\). Rounded to 10 decimal places, the numerical approximation is \(0.0000000000\).

{"answer": "0", "numerical_answer": "0.0000000000"}