# Evaluating $\int\limits_0^2 x^{1/2}(2-x)^{-1/2}\cosh\left(\sqrt{x(2-x)}\right)dx$

I'll solve this definite integral through substitution and properties of hyperbolic functions.

## Step 1: Consider a substitution
Let's use the substitution $u = \sqrt{x(2-x)}$. First, I'll find the relationship between $x$ and $u$.

We have:
$u^2 = x(2-x) = 2x - x^2$

Now I need to express $x$ in terms of $u$. Let's rearrange:
$x^2 - 2x + u^2 = 0$

Using the quadratic formula:
$x = \frac{2 \pm \sqrt{4-4u^2}}{2} = 1 \pm \sqrt{1-u^2}$

Since we're integrating from $x=0$ to $x=2$, and $u = \sqrt{x(2-x)}$ needs to be defined in this range, we'll use:
$x = 1 - \sqrt{1-u^2}$ when $x < 1$
$x = 1 + \sqrt{1-u^2}$ when $x > 1$

But notice that $u = \sqrt{x(2-x)}$ is symmetric about $x=1$. When $x=0$, $u=0$, and when $x=2$, $u=0$ as well. At $x=1$, $u=1$.

## Step 2: Compute the derivative for substitution
Since $u^2 = x(2-x)$, differentiating both sides:
$2u\frac{du}{dx} = 2 - 2x$
$\frac{du}{dx} = \frac{2-2x}{2u} = \frac{1-x}{u}$

Therefore:
$dx = \frac{u}{1-x}du$

## Step 3: Express the integrand in terms of $u$
We need to rewrite $x^{1/2}(2-x)^{-1/2}$ in terms of $u$.

$x(2-x) = u^2$ implies $2-x = \frac{u^2}{x}$
So $(2-x)^{-1/2} = \left(\frac{u^2}{x}\right)^{-1/2} = \frac{x^{1/2}}{u}$

Therefore, $x^{1/2}(2-x)^{-1/2} = x^{1/2} \cdot \frac{x^{1/2}}{u} = \frac{x}{u}$

## Step 4: Transform the integral

Now the integral becomes:
$\int_0^2 x^{1/2}(2-x)^{-1/2}\cosh\left(\sqrt{x(2-x)}\right)dx = \int_0^2 \frac{x}{u}\cosh(u)\frac{u}{1-x}du = \int_0^2 \frac{x}{1-x}\cosh(u)du$

But there's a challenge: we have a mix of $x$ and $u$ variables. Let's approach this differently.

## Alternative approach
Let's use a symmetry property. Notice that our integral is over $[0,2]$ and $x(2-x)$ is symmetric about $x=1$.

Let's split the integral at $x=1$:
$\int_0^2 x^{1/2}(2-x)^{-1/2}\cosh\left(\sqrt{x(2-x)}\right)dx = \int_0^1 x^{1/2}(2-x)^{-1/2}\cosh\left(\sqrt{x(2-x)}\right)dx + \int_1^2 x^{1/2}(2-x)^{-1/2}\cosh\left(\sqrt{x(2-x)}\right)dx$

For the second integral, let's substitute $y = 2-x$, which gives $dx = -dy$ and transforms the limits:
$\int_1^2 x^{1/2}(2-x)^{-1/2}\cosh\left(\sqrt{x(2-x)}\right)dx = -\int_1^0 (2-y)^{1/2}y^{-1/2}\cosh\left(\sqrt{y(2-y)}\right)dy = \int_0^1 (2-y)^{1/2}y^{-1/2}\cosh\left(\sqrt{y(2-y)}\right)dy$

Now, the combined integral is:
$\int_0^1 [x^{1/2}(2-x)^{-1/2} + (2-x)^{1/2}x^{-1/2}]\cosh\left(\sqrt{x(2-x)}\right)dx$

Let's simplify the factor in brackets:
$x^{1/2}(2-x)^{-1/2} + (2-x)^{1/2}x^{-1/2} = \frac{x}{(x(2-x))^{1/2}} + \frac{2-x}{(x(2-x))^{1/2}} = \frac{2}{(x(2-x))^{1/2}} = \frac{2}{\sqrt{x(2-x)}}$

So our integral becomes:
$\int_0^1 \frac{2}{\sqrt{x(2-x)}}\cosh\left(\sqrt{x(2-x)}\right)dx$

Now let's use the substitution $u = \sqrt{x(2-x)}$ again:
When $x=0$, $u=0$; when $x=1$, $u=1$.

From $u^2 = x(2-x)$, we get:
$2u\frac{du}{dx} = 2 - 2x$
$dx = \frac{u}{1-x}du$

But we need to express $\frac{1}{\sqrt{x(2-x)}}$ in terms of $u$:
$\frac{1}{\sqrt{x(2-x)}} = \frac{1}{u}$

So our integral becomes:
$\int_0^1 \frac{2}{u}\cosh(u)\frac{u}{1-x}du = \int_0^1 \frac{2}{1-x}\cosh(u)du$

We still have the challenge of the mixed variables. Let's try yet another approach.

## Final approach
Let's use the substitution $x = 1-\cos\theta$ for $0 \leq \theta \leq \pi$. This maps $x=0$ to $\theta=0$ and $x=2$ to $\theta=\pi$.

With this substitution:
$2-x = 2-(1-\cos\theta) = 1+\cos\theta$
$x(2-x) = (1-\cos\theta)(1+\cos\theta) = 1-\cos^2\theta = \sin^2\theta$
$\sqrt{x(2-x)} = \sin\theta$

Also:
$dx = \sin\theta d\theta$
$x^{1/2} = (1-\cos\theta)^{1/2}$
$(2-x)^{-1/2} = (1+\cos\theta)^{-1/2}$

The integral becomes:
$\int_0^\pi (1-\cos\theta)^{1/2}(1+\cos\theta)^{-1/2}\cosh(\sin\theta)\sin\theta d\theta$

Let's simplify:
$(1-\cos\theta)^{1/2}(1+\cos\theta)^{-1/2} = \sqrt{\frac{1-\cos\theta}{1+\cos\theta}} = \sqrt{\frac{(1-\cos\theta)^2}{(1-\cos\theta)(1+\cos\theta)}} = \frac{1-\cos\theta}{\sin\theta}$

So the integral is:
$\int_0^\pi \frac{1-\cos\theta}{\sin\theta}\cosh(\sin\theta)\sin\theta d\theta = \int_0^\pi (1-\cos\theta)\cosh(\sin\theta) d\theta$

Now we can split this into two parts:
$\int_0^\pi \cosh(\sin\theta) d\theta - \int_0^\pi \cos\theta\cosh(\sin\theta) d\theta$

For the first part, note that $\cosh(\sin\theta)$ is even in $\theta$ with respect to $\theta=\pi/2$, so:
$\int_0^\pi \cosh(\sin\theta) d\theta = 2\int_0^{\pi/2} \cosh(\sin\theta) d\theta$

For the second part, let's use integration by parts:
$\int \cos\theta\cosh(\sin\theta) d\theta$
Let $u = \cos\theta$ and $dv = \cosh(\sin\theta) d\theta$
Then $du = -\sin\theta d\theta$ and $v = \sinh(\sin\theta)$

So:
$\int \cos\theta\cosh(\sin\theta) d\theta = \cos\theta\sinh(\sin\theta) + \int \sin\theta\sinh(\sin\theta) d\theta$

For the remaining integral, with $w = \sin\theta$, $dw = \cos\theta d\theta$:
$\int \sin\theta\sinh(\sin\theta) d\theta = \int \sin\theta\sinh(w)\frac{dw}{\cos\theta} = \int w\sinh(w) \frac{1}{\sqrt{1-w^2}} dw$

Actually, let's restart with a more direct approach.

## Direct approach
The given integral is:
$\int_0^2 x^{1/2}(2-x)^{-1/2}\cosh\left(\sqrt{x(2-x)}\right)dx$

I'll use the substitution $x = 1-\cos\theta$ for $0 \leq \theta \leq \pi$.
This gives:
- $dx = \sin\theta d\theta$
- $2-x = 1+\cos\theta$
- $\sqrt{x(2-x)} = \sin\theta$

The integral becomes:
$\int_0^\pi (1-\cos\theta)^{1/2}(1+\cos\theta)^{-1/2}\cosh(\sin\theta)\sin\theta d\theta$

We can simplify:
$(1-\cos\theta)^{1/2} = \sqrt{2}\sin(\theta/2)$
$(1+\cos\theta)^{-1/2} = \frac{1}{\sqrt{2}\cos(\theta/2)}$

So:
$(1-\cos\theta)^{1/2}(1+\cos\theta)^{-1/2} = \frac{\sin(\theta/2)}{\cos(\theta/2)} = \tan(\theta/2)$

The integral becomes:
$\int_0^\pi \tan(\theta/2)\cosh(\sin\theta)\sin\theta d\theta$

Using the identity $\sin\theta = 2\sin(\theta/2)\cos(\theta/2)$, we get:
$\tan(\theta/2)\sin\theta = 2\sin^2(\theta/2)$

So our integral is:
$\int_0^\pi 2\sin^2(\theta/2)\cosh(\sin\theta) d\theta$

Using the half-angle formula $\sin^2(\theta/2