Let's compute the definite integral:
\[
I = \int_0^\pi \sec x \ln\left(1+\frac{\cos x}{3}\right) dx
\]

**Step 1: Symmetry Analysis and Substitution**

Let’s use the substitution \( x \rightarrow \pi - x \):

- \(\cos(\pi - x) = -\cos x\)
- \(\sec(\pi - x) = -\sec x\)

So,
\[
I = \int_0^\pi \sec(\pi-x) \ln\left(1+\frac{\cos(\pi-x)}{3}\right) dx = \int_0^\pi [-\sec x] \ln\left(1-\frac{\cos x}{3}\right) dx
\]
\[
I = -\int_0^\pi \sec x \ln\left(1-\frac{\cos x}{3}\right) dx
\]

So, the original integral plus this transformed integral gives:

\[
I + I' = \int_0^\pi \sec x \left[ \ln\left(1+\frac{\cos x}{3}\right) - \ln\left(1-\frac{\cos x}{3}\right) \right] dx
\]
\[
= \int_0^\pi \sec x \ln\left( \frac{1+\frac{\cos x}{3}}{1-\frac{\cos x}{3}} \right) dx
\]

But note that \( I' = -I \), so:
\[
I + (-I) = [\text{expression above}]
\]
\[
0 = \int_0^\pi \sec x \ln\left( \frac{1+\frac{\cos x}{3}}{1-\frac{\cos x}{3}} \right) dx
\]
Therefore,
\[
\int_0^\pi \sec x \ln\left( \frac{1+\frac{\cos x}{3}}{1-\frac{\cos x}{3}} \right) dx = 0
\]

Alternatively, express \( I \) as an average:
\[
I = \frac{1}{2} \int_0^\pi \sec x \ln\left( \frac{1+\frac{\cos x}{3}}{1-\frac{\cos x}{3}} \right) dx
\]
\[
= \frac{1}{2} \cdot 0 = 0
\]

But this can't be: let's double-check the steps.

**Step 2: Series Expansion**

Expand \(\ln\left(1+\frac{\cos x}{3}\right)\) as a Taylor series:
\[
\ln(1 + y) = \sum_{n=1}^\infty \frac{(-1)^{n+1}}{n} y^n
\]
Therefore,
\[
\ln\left(1+\frac{\cos x}{3}\right) = \sum_{n=1}^\infty \frac{(-1)^{n+1}}{n} \left(\frac{\cos x}{3}\right)^n
\]

Plug this into the integral:
\[
I = \int_0^\pi \sec x \sum_{n=1}^\infty \frac{(-1)^{n+1}}{n} \left(\frac{\cos x}{3}\right)^n dx
\]
\[
= \sum_{n=1}^\infty \frac{(-1)^{n+1}}{n 3^n} \int_0^\pi \sec x (\cos x)^n dx
\]
\[
= \sum_{n=1}^\infty \frac{(-1)^{n+1}}{n 3^n} \int_0^\pi (\cos x)^{n} \sec x dx
\]
But \(\sec x (\cos x)^n = (\cos x)^{n-1}\). Therefore,
\[
I = \sum_{n=1}^\infty \frac{(-1)^{n+1}}{n 3^n} \int_0^\pi (\cos x)^{n-1} dx
\]

**Step 3: Integrating \(\int_0^\pi (\cos x)^{n-1} dx\)**

Let’s denote:
\[
J_m = \int_0^\pi (\cos x)^m dx
\]
It is known that:
- For odd \(m\) (\(m=2k+1\)), \(J_{2k+1}=0\).
- For even \(m\) (\(m=2k\)), \(J_{2k} = \pi \dfrac{(2k)!}{2^{2k} (k!)^2}\)

But, more precisely,
\[
\int_0^\pi (\cos x)^m dx = 
\begin{cases}
\pi \binom{m}{m/2} \frac{1}{2^m}, & \text{if $m$ even} \\
0, & \text{if $m$ odd}
\end{cases}
\]

So, set \(n-1 = m\).
- If \(m=2k\), \(n = 2k+1\), odd.
- If \(m=2k+1\), \(n=2k+2\), even.

So, only the even powers contribute (since the integral is 0 for odd powers).

Therefore, the only nonzero contributions are for \(n\) **even**, namely, \(n = 2k\), \(k \geq 1\).

So,
\[
I = \sum_{k=1}^{\infty} \frac{(-1)^{2k+1}}{2k \cdot 3^{2k}} J_{2k-1}
\]
But \(J_{2k-1} = 0\), so only \(J_{2k}\) contribute, that is,
let's write as:

\[
I = \sum_{k=0}^\infty \frac{(-1)^{2k+2}}{(2k+2) 3^{2k+2}} J_{2k+1}
\]
But \(J_{2k+1} = 0\).

Alternatively, sum over odd \(n = 2k+1\):
\[
I = \sum_{k=0}^\infty \frac{(-1)^{2k+2}}{(2k+2)3^{2k+2}} J_{2k+1} = 0
\]

Thus, **the only nonzero \(J_m\) are for even powers. In our case, the powers are always odd, so the integral evaluates to zero.**

**Step 4: Final Evaluation**

Thus,
\[
\boxed{I = 0}
\]

**Numerical value:** \(0.0000000000\)

**JSON output:**
```json
{"answer": "0", "numerical_answer": "0.0000000000"}
```