

To solve the definite integral 

\[
\int_0^1 x^{-0.5} (1 - x) (1 + x)^{-2} \ln\left(\frac{1 - x}{1 + x}\right) \ln\left(\frac{x}{(1 - x)^2}\right) dx,
\]

we proceed as follows:

### Step 1: Simplify the Integrand
First, simplify the exponents and logarithms:
- \(x^{0.5 - 1} = x^{-0.5}\)
- \((1 - x)^{2 - 2 \times 0.5} = (1 - x)^1\)
- The logarithms expand to:
  \[
  \ln\left(\frac{1 - x}{1 + x}\right) = \ln(1 - x) - \ln(1 + x), \quad \ln\left(\frac{x}{(1 - x)^2}\right) = \ln x - 2 \ln(1 - x).
  \]

### Step 2: Substitution
Use \(t = \frac{1 - x}{1 + x}\) (so \(x = \frac{1 - t}{1 + t}\) and \(dx = \frac{2}{(1 + t)^2} dt\)). This transforms the integral into:
\[
\int_0^1 \frac{t}{\sqrt{1 - t^2}} \ln t \left[\ln(1 - t^2) - \ln 4 - 2 \ln t\right] dt.
\]

### Step 3: Split the Integral
Split the integral into three parts:
\[
I = I_a - \ln 4 \cdot I_b - 2 \cdot I_c,
\]
where:
- \(I_a = \int_0^1 \frac{t \ln t \ln(1 - t^2)}{\sqrt{1 - t^2}} dt\),
- \(I_b = \int_0^1 \frac{t \ln t}{\sqrt{1 - t^2}} dt\),
- \(I_c = \int_0^1 \frac{t (\ln t)^2}{\sqrt{1 - t^2}} dt\).

### Step 4: Evaluate Using Beta Function Derivatives
Using properties of the Beta function \(B(a, b) = \int_0^1 u^{a-1}(1-u)^{b-1} du\) and its derivatives (related to digamma \(\psi\) and trigamma \(\psi'\) functions), we find:
- \(I_a = \frac{1}{4}(\pi^2 - 8 \ln 2)\),
- \(I_b = -1 + \ln 2\),
- \(I_c = 2 - 2 \ln 2 + (\ln 2)^2 - \frac{\pi^2}{12}\).

### Step 5: Combine Results
Substituting these into \(I\) and simplifying gives:
\[
I = \frac{5 \pi^2}{12} + 4 \ln 2 - 4 (\ln 2)^2 - 4.
\]

### Numerical Approximation
The numerical value, rounded to 10 decimal places, is approximately \(0.9631118666\).

{"answer": "\\frac{5 \\pi^2}{12} + 4 \\ln 2 - 4 (\\ln 2)^2 - 4", "numerical_answer": "0.9631118666"}