

To calculate the definite integral \(\int_1^e x (\log x)^2 \, dx\), we use integration by parts.

### Step 1: First Integration by Parts
Let \( u = (\log x)^2 \) and \( dv = x \, dx \). Then:
- \( du = 2 \log x \cdot \frac{1}{x} \, dx \)
- \( v = \int x \, dx = \frac{1}{2}x^2 \)

By integration by parts:
\[
\int x (\log x)^2 \, dx = uv - \int v \, du = \frac{1}{2}x^2 (\log x)^2 - \int \frac{1}{2}x^2 \cdot 2 \log x \cdot \frac{1}{x} \, dx
\]
Simplifying the remaining integral:
\[
\int x (\log x)^2 \, dx = \frac{1}{2}x^2 (\log x)^2 - \int x \log x \, dx
\]

### Step 2: Second Integration by Parts (for \(\int x \log x \, dx\))
Let \( u = \log x \) and \( dv = x \, dx \). Then:
- \( du = \frac{1}{x} \, dx \)
- \( v = \frac{1}{2}x^2 \)

By integration by parts:
\[
\int x \log x \, dx = \frac{1}{2}x^2 \log x - \int \frac{1}{2}x^2 \cdot \frac{1}{x} \, dx = \frac{1}{2}x^2 \log x - \frac{1}{2} \int x \, dx
\]
Simplifying the remaining integral:
\[
\int x \log x \, dx = \frac{1}{2}x^2 \log x - \frac{1}{4}x^2 + C
\]

### Step 3: Evaluate the Definite Integral
Combining the results and evaluating from \(1\) to \(e\):
\[
\int_1^e x (\log x)^2 \, dx = \left[ \frac{1}{2}x^2 (\log x)^2 \right]_1^e - \left[ \frac{1}{2}x^2 \log x - \frac{1}{4}x^2 \right]_1^e
\]

- For the first term \(\left[ \frac{1}{2}x^2 (\log x)^2 \right]_1^e\):
  - At \(x = e\): \(\frac{1}{2}e^2 (\log e)^2 = \frac{1}{2}e^2\)
  - At \(x = 1\): \(\frac{1}{2}(1)^2 (\log 1)^2 = 0\)
  - Result: \(\frac{1}{2}e^2 - 0 = \frac{1}{2}e^2\)

- For the second term \(\left[ \frac{1}{2}x^2 \log x - \frac{1}{4}x^2 \right]_1^e\):
  - At \(x = e\): \(\frac{1}{2}e^2 \log e - \frac{1}{4}e^2 = \frac{1}{2}e^2 - \frac{1}{4}e^2 = \frac{1}{4}e^2\)
  - At \(x = 1\): \(\frac{1}{2}(1)^2 \log 1 - \frac{1}{4}(1)^2 = 0 - \frac{1}{4} = -\frac{1}{4}\)
  - Result: \(\frac{1}{4}e^2 - \left(-\frac{1}{4}\right) = \frac{1}{4}e^2 + \frac{1}{4}\)

### Final Result
Subtracting the second term from the first:
\[
\int_1^e x (\log x)^2 \, dx = \frac{1}{2}e^2 - \left( \frac{1}{4}e^2 + \frac{1}{4} \right) = \frac{1}{4}e^2 - \frac{1}{4} = \frac{e^2 - 1}{4}
\]

### Numerical Approximation
Using \(e \approx 2.718281828459045\), we compute \(e^2 \approx 7.3890560989306495\). Thus:
\[
\frac{e^2 - 1}{4} \approx \frac{7.3890560989306495 - 1}{4} \approx \frac{6.3890560989306495}{4} \approx 1.5972640247
\]

{"answer": "\\frac{e^2 - 1}{4}", "numerical_answer": "1.5972640247"}