To solve the definite integral \(\int_0^{\pi/4}\frac{\tan(x)+2\sec^2(x)+2\tan(x)\sec^2(x)}{\tan(x)+\sec^2(x)}\, dx\), we start by simplifying the integrand.

First, let's rewrite the integrand:
\[
\frac{\tan(x) + 2\sec^2(x) + 2\tan(x)\sec^2(x)}{\tan(x) + \sec^2(x)}
\]

We can factor out \(\sec^2(x)\) from the numerator:
\[
\tan(x) + 2\sec^2(x) + 2\tan(x)\sec^2(x) = \tan(x) + 2\sec^2(x)(1 + \tan(x))
\]

Thus, the integrand becomes:
\[
\frac{\tan(x) + 2\sec^2(x)(1 + \tan(x))}{\tan(x) + \sec^2(x)}
\]

We can split this into two fractions:
\[
\frac{\tan(x)}{\tan(x) + \sec^2(x)} + \frac{2\sec^2(x)(1 + \tan(x))}{\tan(x) + \sec^2(x)}
\]

Notice that:
\[
\frac{\tan(x)}{\tan(x) + \sec^2(x)} + \frac{2\sec^2(x)(1 + \tan(x))}{\tan(x) + \sec^2(x)} = 1 + \frac{\sec^2(x)}{\tan(x) + \sec^2(x)}
\]

So, the integral simplifies to:
\[
\int_0^{\pi/4} \left(1 + \frac{\sec^2(x)}{\tan(x) + \sec^2(x)}\right) \, dx
\]

This can be split into two integrals:
\[
\int_0^{\pi/4} 1 \, dx + \int_0^{\pi/4} \frac{\sec^2(x)}{\tan(x) + \sec^2(x)} \, dx
\]

The first integral is straightforward:
\[
\int_0^{\pi/4} 1 \, dx = \left. x \right|_0^{\pi/4} = \frac{\pi}{4}
\]

For the second integral, let \(u = \tan(x)\). Then \(du = \sec^2(x) \, dx\). When \(x = 0\), \(u = 0\), and when \(x = \frac{\pi}{4}\), \(u = 1\). The integral becomes:
\[
\int_0^1 \frac{1}{u + 1 + u^2} \, du
\]

We can simplify the denominator:
\[
u + 1 + u^2 = u^2 + u + 1
\]

Thus, the integral is:
\[
\int_0^1 \frac{1}{u^2 + u + 1} \, du
\]

To solve this, we complete the square in the denominator:
\[
u^2 + u + 1 = \left(u + \frac{1}{2}\right)^2 + \frac{3}{4}
\]

So the integral becomes:
\[
\int_0^1 \frac{1}{\left(u + \frac{1}{2}\right)^2 + \frac{3}{4}} \, du
\]

Let \(v = u + \frac{1}{2}\). Then \(dv = du\). When \(u = 0\), \(v = \frac{1}{2}\), and when \(u = 1\), \(v = \frac{3}{2}\). The integral becomes:
\[
\int_{1/2}^{3/2} \frac{1}{v^2 + \frac{3}{4}} \, dv
\]

This is a standard form of the arctangent integral:
\[
\int \frac{1}{v^2 + a^2} \, dv = \frac{1}{a} \arctan\left(\frac{v}{a}\right) + C
\]

Here, \(a = \frac{\sqrt{3}}{2}\), so:
\[
\int_{1/2}^{3/2} \frac{1}{v^2 + \frac{3}{4}} \, dv = \frac{2}{\sqrt{3}} \left[ \arctan\left(\frac{2v}{\sqrt{3}}\right) \right]_{1/2}^{3/2}
\]

Evaluating this:
\[
\frac{2}{\sqrt{3}} \left( \arctan\left(\frac{3}{\sqrt{3}}\right) - \arctan\left(\frac{1}{\sqrt{3}}\right) \right) = \frac{2}{\sqrt{3}} \left( \arctan(\sqrt{3}) - \arctan\left(\frac{1}{\sqrt{3}}\right) \right)
\]

Since \(\arctan(\sqrt{3}) = \frac{\pi}{3}\) and \(\arctan\left(\frac{1}{\sqrt{3}}\right) = \frac{\pi}{6}\):
\[
\frac{2}{\sqrt{3}} \left( \frac{\pi}{3} - \frac{\pi}{6} \right) = \frac{2}{\sqrt{3}} \cdot \frac{\pi}{6} = \frac{\pi}{3\sqrt{3}} = \frac{\pi \sqrt{3}}{9}
\]

Combining both parts of the integral:
\[
\frac{\pi}{4} + \frac{\pi \sqrt{3}}{9}
\]

Thus, the exact answer is:
\[
\frac{\pi}{4} + \frac{\pi \sqrt{3}}{9}
\]

Numerically, this is approximately:
\[
\frac{\pi}{4} \approx 0.7853981634
\]
\[
\frac{\pi \sqrt{3}}{9} \approx 0.6045997880
\]
\[
0.7853981634 + 0.6045997880 \approx 1.3899979514
\]

Rounded to 10 decimal places, the numerical approximation is:
\[
1.3899979514
\]

Finally, the answer in the required JSON format is:
```json
{"answer": "\\frac{\\pi}{4} + \\frac{\\pi \\sqrt{3}}{9}", "numerical_answer": "1.3899979514"}
```