Let's proceed step by step.

## 1. Compute the integral analytically

Given:
\[
I = \int_{64}^{729} \frac{x^{1/2}}{x^{1/2}-x^{1/3}} \, dx
\]

Let's factor out \( x^{1/2} \):

\[
\frac{x^{1/2}}{x^{1/2} - x^{1/3}} = \frac{1}{1 - x^{-1/6}}
\]

because
\[
x^{1/2} - x^{1/3} = x^{1/2}(1 - x^{-1/6})
\implies \frac{x^{1/2}}{x^{1/2} - x^{1/3}} = \frac{1}{1 - x^{-1/6}}
\]

So,
\[
I = \int_{64}^{729} \frac{1}{1 - x^{-1/6}} dx
\]

Let’s perform a substitution to simplify.

Let \( u = x^{1/6} \implies x = u^6 \)
Then \( dx = 6 u^5 du \)

When \( x = 64 = 2^6 \implies u = 2 \)
When \( x = 729 = 3^6 \implies u = 3 \)

Also, \( x^{-1/6} = u^{-1} \)

Thus,
\[
I = \int_{x=64}^{x=729} \frac{1}{1 - x^{-1/6}} dx 
= \int_{u=2}^{u=3} \frac{1}{1-u^{-1}} \cdot dx 
\]
But \( 1-u^{-1} = \frac{u-1}{u} \implies \frac{1}{1-u^{-1}} = \frac{u}{u-1} \)

So,
\[
\frac{1}{1-u^{-1}} \cdot dx = \frac{u}{u-1} \cdot 6u^5 du = 6\frac{u^6}{u-1} du
\]

Therefore,
\[
I = 6 \int_{u=2}^{u=3} \frac{u^6}{u-1} du
\]

Let's write \( u^6 = (u-1+1)^6 \) if we want to expand, but better to use polynomial division:

\[
\frac{u^6}{u-1}
\]

We perform polynomial long division:

Divide \( u^6 \) by \( u-1 \):

\[
u^6 = (u-1) Q(u) + R
\]
The quotient will be \( u^5 + u^4 + u^3 + u^2 + u + 1 \), the remainder is 1.

Because:
\[
(u-1)(u^5 + u^4 + u^3 + u^2 + u + 1) = u^6 - u^5 + u^5 - u^4 + u^4 - u^3 + u^3 - u^2 + u^2 - u + u - 1
\]
So all interior terms cancel and we get:
\[
(u-1)(u^5 + u^4 + u^3 + u^2 + u + 1) = u^6 - 1
\]
So,
\[
u^6 = (u-1)(u^5 + u^4 + u^3 + u^2 + u + 1) + 1
\]
Therefore,
\[
\frac{u^6}{u-1} = u^5 + u^4 + u^3 + u^2 + u + 1 + \frac{1}{u-1}
\]

Putting it together:
\[
I = 6 \int_{u=2}^{u=3} \left( u^5 + u^4 + u^3 + u^2 + u + 1 + \frac{1}{u-1} \right) du
\]

Let's integrate each term:

- \( \int u^5 du = \frac{u^6}{6} \)
- \( \int u^4 du = \frac{u^5}{5} \)
- \( \int u^3 du = \frac{u^4}{4} \)
- \( \int u^2 du = \frac{u^3}{3} \)
- \( \int u du = \frac{u^2}{2} \)
- \( \int 1 du = u \)
- \( \int \frac{1}{u-1} du = \ln|u-1| \)

Thus,
\[
I =6 \left. \left[ \frac{u^6}{6} + \frac{u^5}{5} + \frac{u^4}{4} + \frac{u^3}{3} + \frac{u^2}{2} + u + \ln|u-1| \right] \right|_{u=2}^{u=3}
\]

Let’s simplify:

Multiplying terms by 6:

- \( 6 \times \frac{u^6}{6} = u^6 \)
- \( 6 \times \frac{u^5}{5} = \frac{6u^5}{5} \)
- \( 6 \times \frac{u^4}{4} = \frac{3u^4}{2} \)
- \( 6 \times \frac{u^3}{3} = 2u^3 \)
- \( 6 \times \frac{u^2}{2} = 3u^2 \)
- \( 6 \times u = 6u \)
- \( 6 \times \ln|u-1| = 6\ln|u-1| \)

So:
\[
I = \left. \left[ u^6 + \frac{6u^5}{5} + \frac{3u^4}{2} + 2u^3 + 3u^2 + 6u + 6\ln|u-1| \right] \right|_{2}^{3}
\]

## 2. Plug in the limits

### At \( u = 3 \):

- \( 3^6 = 729 \)
- \( 6 \cdot 3^5 = 6 \cdot 243 = 1458 \), so \( 1458/5 \)
- \( 3^4 = 81 \), \( 3 \cdot 81 = 243 \), so \( 243/2 \)
- \( 2 \cdot 3^3 = 2 \cdot 27 = 54 \)
- \( 3 \cdot 3^2 = 3 \cdot 9 = 27 \)
- \( 6 \cdot 3 = 18 \)
- \( 6\ln(3-1) = 6\ln 2 \)

So sum at \( u = 3 \):

\[
\begin{align*}
A = &\ 729 \\
& + \frac{1458}{5} \\
& + \frac{243}{2} \\
& + 54 \\
& + 27 \\
& + 18 \\
& + 6\ln 2 \\
\end{align*}
\]

### At \( u = 2 \):

- \( 2^6 = 64 \)
- \( 6\cdot 2^5 = 6 \cdot 32 = 192 \), so \( 192/5 \)
- \( 2^4 = 16 \), \( 3\cdot 16 = 48 \), \( 48/2 = 24 \)
- \( 2\cdot 2^3 = 2 \cdot 8 = 16 \)
- \( 3\cdot 2^2 = 3 \cdot 4 = 12 \)
- \( 6 \cdot 2 = 12 \)
- \( 6\ln(2-1) = 6\ln 1 = 0 \)

So sum at \( u = 2 \):

\[
\begin{align*}
B =&\ 64 \\
& + \frac{192}{5} \\
& + 24 \\
& + 16 \\
& + 12 \\
& + 12 \\
& + 0 \\
\end{align*}
\]

Therefore:
\[
I = (A) - (B)
\]

Let’s write the explicit expression:

\[
I = 
\bigg[729 + \frac{1458}{5} + \frac{243}{2} + 54 + 27 + 18 + 6 \ln 2\bigg]
- \bigg[64 + \frac{192}{5} + 24 + 16 + 12 + 12 \bigg]
\]

Let’s compute each term:

### 2a. Compute numerators and denominators

#### Numerically:

**Upper limit sum:**

- \( 729 \)
- \( 1458 / 5 = 291.6 \)
- \( 243 / 2 = 121.5 \)
- \( 54 \)
- \( 27 \)
- \( 18 \)
- \( 6 \ln 2 \approx 6 \cdot 0.6931471806 = 4.1588830836 \)
- Sum: \( 729 + 291.6 + 121.5 + 54 + 27 + 18 + 4.1588830836 \)

Let’s add step by step:

- \( 729 + 291.6 = 1020.6 \)
- \( 1020.6 + 121.5 = 1142.1 \)
- \( 1142.1 + 54 = 1196.1 \)
- \( 1196.1 + 27 = 1223.1 \)
- \( 1223.1 + 18 = 1241.1 \)
- \( 1241.1 + 4.1588830836 = 1245.2588830836 \)

**Lower limit sum:**

- \( 64 \)
- \( 192 / 5 = 38.4 \)
- \( 24 \)
- \( 16 \)
- \( 12 \)
- \( 12 \)
- Sum: \( 64 + 38.4 + 24 + 16 + 12 + 12 \)

Sum step by step:

- \( 64 + 38.4 = 102.4 \)
- \( 102.4 + 24 = 126.4 \)
- \( 126.4 + 16 = 142.4 \)
- \( 142.4 + 12 = 154.4 \)
- \( 154.4 + 12 = 166.4 \)

Therefore,

\[
I = 1245.2588830836 - 166.4 = 1078.8588830836
\]

Rounding to 10 decimal places: \( 1078.8588830836 \)

## 3. Exact answer in LaTeX

So the **exact value** is:

\[
I = \left[729 + \frac{1458}{5} + \frac{243}{2} + 54 + 27 + 18 + 6\ln 2\right] - \left[64 + \frac{192}{5} + 24 + 16 + 12 + 12\right]
\]

Or, factoring:

\[
I = \left(729 - 64 \right)
  + \left(\frac{1458}{5} - \frac{192}{5}\right)
  + \left(\frac{243}{2} - 24\right)
  + (54 - 16)
  + (27 - 12)
  + (18 - 12)
  + 6\ln 2
\]

You may also write:

\[
I = 665 + \frac{1266}{5} + \frac{195}{2} + 38 + 15 + 6 + 6\ln 2
\]
But since the original request is for the full upper and lower expressions, I'll use the larger version.

## 4. JSON output

Final answer, formatted as requested:

```json
{"answer": "\\left[729 + \\frac{1458}{5} + \\frac{243}{2} + 54 + 27 + 18 + 6\\ln 2\\right] - \\left[64 + \\frac{192}{5} + 24 + 16 + 12 + 12\\right]", "numerical_answer": "1078.8588830836"}
```