We start with the integral

  I = ∫₀² x^(–1/2) (2–x)^(1/2) [1 – 0.5 x (2–x)]^(1/2) dx.

Step 1. A change of variable

Let
  x = 2 sin²θ     so that dx = 4 sinθ cosθ dθ.
When x = 0, θ = 0; when x = 2, sin²θ = 1 so that θ = π/2.

Now compute the factors:
• x^(–1/2) = (2 sin²θ)^(–1/2) = 1/(√2 sinθ).
• (2–x)^(1/2) = (2 – 2 sin²θ)^(1/2) = (2 cos²θ)^(1/2) = √2 cosθ.
Thus, 
  x^(–1/2)(2–x)^(1/2) = (1/(√2 sinθ))·(√2 cosθ) = cotθ.

Also, note that
  x(2–x) = (2 sin²θ)(2 cos²θ) = 4 sin²θ cos²θ,
so that
  0.5 x(2–x) = 0.5·4 sin²θ cos²θ = 2 sin²θ cos²θ.
Then the last factor becomes
  [1 – 0.5 x(2–x)]^(1/2) = [1 – 2 sin²θ cos²θ]^(1/2).
But since sin(2θ) = 2 sinθ cosθ, we have sin²(2θ) = 4 sin²θ cos²θ and hence
  2 sin²θ cos²θ = (1/2) sin²(2θ).
Thus, the last factor is
  √[1 – (1/2) sin²(2θ)].

Also, the differential is dx = 4 sinθ cosθ dθ.

Altogether the integrand in terms of θ becomes:
  I = ∫₀^(π/2) (cotθ) · √[1 – (1/2) sin²(2θ)] · (4 sinθ cosθ dθ).

Since cotθ = cosθ/sinθ, we combine:
  cotθ · (4 sinθ cosθ) = 4 cos²θ.
Thus,
  I = 4 ∫₀^(π/2) cos²θ √[1 – (1/2) sin²(2θ)] dθ.

Step 2. Changing the variable to double the angle

Set u = 2θ so that dθ = du/2. When θ goes from 0 to π/2, u goes from 0 to π.
Note that cos²θ can be written in terms of u:
  cos²θ = cos²(u/2) = (1 + cos u)/2.
Then
  I = 4 ∫₀^(π/2) cos²θ √[1 – (1/2) sin²(2θ)] dθ
    = 4 ∫₀^(π) cos²(u/2) √[1 – (1/2) sin² u] · (du/2)
    = 2 ∫₀^(π) cos²(u/2) √[1 – (1/2) sin² u] du
    = 2 ∫₀^(π) (1+cos u)/2 √[1 – (1/2) sin² u] du
    = ∫₀^(π) (1+cos u) √[1 – (1/2) sin² u] du.

Now split the integral:
  I = ∫₀^(π) √[1 – (1/2) sin² u] du  + ∫₀^(π) cos u √[1 – (1/2) sin² u] du.

The second integral vanishes because the integrand is odd (by the change u → π – u, one finds it cancels), so
  I = ∫₀^(π) √[1 – (1/2) sin² u] du.

Because sin²u is symmetric about u = π/2, we can write
  I = 2∫₀^(π/2) √[1 – (1/2) sin² u] du.

Step 3. Recognizing the complete elliptic integral

Recall the definition of the complete elliptic integral of the second kind:
  E(k) = ∫₀^(π/2) √(1 – k² sin² φ) dφ.
Here, if we choose k² = 1/2 (that is, k = 1/√2), then
  E(1/√2) = ∫₀^(π/2) √[1 – (1/2) sin²φ] dφ.
Thus,
  I = 2 E(1/√2).

Step 4. Numerical Approximation

It is known that 
  E(1/√2) ≈ 1.4674622093,
so that
  I ≈ 2 × 1.4674622093 ≈ 2.9349244186.
Rounded to 10 decimal places, this is approximately 2.9349244187.

Final Answer in JSON:
{"answer": "2\\,E\\left(\\frac{1}{\\sqrt{2}}\\right)", "numerical_answer": "2.9349244187"}