
To solve the definite integral \(\int_0^1 x^{-1/4}(1 - x)^{1/4} I_1\left(\sqrt[4]{x(1 - x)}\right) dx\), we proceed as follows:

### Step 1: Series Expansion of the Bessel Function
The modified Bessel function of the first kind \(I_1(z)\) has the power series expansion:
\[
I_1(z) = \sum_{k=0}^\infty \frac{z^{2k+1}}{2^{2k+1} k! (k+1)!}
\]
Substituting \(z = \sqrt[4]{x(1 - x)}\), we get:
\[
I_1\left(\sqrt[4]{x(1 - x)}\right) = \sum_{k=0}^\infty \frac{\left(x(1 - x)\right)^{(2k+1)/4}}{2^{2k+1} k! (k+1)!}
\]

### Step 2: Substitute the Series into the Integral
The integrand becomes:
\[
x^{-1/4}(1 - x)^{1/4} \sum_{k=0}^\infty \frac{\left(x(1 - x)\right)^{(2k+1)/4}}{2^{2k+1} k! (k+1)!}
\]
Combining the powers of \(x\) and \(1 - x\):
\[
x^{-1/4} \cdot x^{(2k+1)/4} = x^{k/2}, \quad (1 - x)^{1/4} \cdot (1 - x)^{(2k+1)/4} = (1 - x)^{(k+1)/2}
\]
Thus, the integral becomes:
\[
\sum_{k=0}^\infty \frac{1}{2^{2k+1} k! (k+1)!} \int_0^1 x^{k/2} (1 - x)^{(k+1)/2} dx
\]

### Step 3: Evaluate the Beta Function
The integral \(\int_0^1 x^{a} (1 - x)^b dx\) is the Beta function \(B(a+1, b+1) = \frac{\Gamma(a+1)\Gamma(b+1)}{\Gamma(a+b+2)}\). Here, \(a = k/2\) and \(b = (k+1)/2\), so:
\[
B\left(\frac{k}{2} + 1, \frac{k+1}{2} + 1\right) = \frac{\Gamma\left(\frac{k+2}{2}\right) \Gamma\left(\frac{k+3}{2}\right)}{\Gamma\left(\frac{2k+5}{2}\right)}
\]

### Step 4: Simplify Using Gamma Function Identities
Using the duplication formula \(\Gamma(z)\Gamma(z+1/2) = 2^{1-2z}\sqrt{\pi}\Gamma(2z)\) and properties of factorials, the Beta function simplifies to a series of terms involving factorials and powers of 2.

### Step 5: Sum the Series
The resulting series converges to a numerical value. Summing the first few terms (up to \(k=5\)) gives a numerical approximation.


### Exact Answer and Numerical Approximation
The exact answer is the infinite series derived from the power series expansion of \(I_1(z)\) and integration term-by-term. The numerical approximation, rounded to 10 decimal places, is approximately \(0.3503003910\).

```json
{"answer": "\\sum_{k=0}^{\\infty} \\frac{2^{2 - k} (k + 1)(k + 2)}{(2k + 4)!}", "numerical_answer": "0.3503003910"}
```