We start by writing the integrand in partial fractions. Notice that

  1/(1 - x²) = 1/[(1 - x)(1 + x)].

We express it as

  A/(1 - x) + B/(1 + x).

Multiplying both sides by (1 - x)(1 + x) gives

  A(1 + x) + B(1 - x) = 1.

Expanding, we have

  A + Ax + B - Bx = (A + B) + (A - B)x = 1.

Equating coefficients for like powers of x, we require:
  A + B = 1  (constant term),
  A - B = 0  (coefficient of x).

Thus, A = B = 1/2.

The integral becomes

  ∫[1/(1 - x²)] dx = (1/2) ∫[1/(1 - x) + 1/(1 + x)] dx.

Integrate term by term:
  ∫1/(1 - x) dx = -ln|1 - x|       and   ∫1/(1 + x) dx = ln|1 + x|.

Therefore, the antiderivative is

  (1/2)[ln|1 + x| - ln|1 - x|] + C = (1/2) ln|(1 + x)/(1 - x)| + C.

Now, evaluate the definite integral from x = -1/2 to x = 1/2:

  I = [1/2 ln|(1 + x)/(1 - x)|] (from -1/2 to 1/2)
    = (1/2) [ ln((1 + 1/2)/(1 - 1/2)) - ln((1 - 1/2)/(1 + 1/2)) ].

Compute the expressions inside the logarithms:
  At x = 1/2: (1 + 1/2)/(1 - 1/2) = (3/2)/(1/2) = 3.
  At x = -1/2: (1 - 1/2)/(1 + 1/2) = (1/2)/(3/2) = 1/3.

Thus,

  I = (1/2)[ ln(3) - ln(1/3) ] = (1/2)[ ln(3) + ln(3) ] = (1/2)[ 2 ln(3) ] = ln(3).

A numerical approximation of ln(3) is approximately 1.0986122887 when rounded to 10 decimal places.

{"answer": "\\ln(3)", "numerical_answer": "1.0986122887"}