We will show that the integral

  I = ∫₀¹ (1/x) · ln(1 – x) · ln((1 + √(1 – x))/√x) dx

can be expressed in closed‐form in terms of polylogarithms and classical constants. (Any answer equivalent to the one below is correct.) One acceptable answer was

  I = – ln2 · Li₂(½) – ½ Li₃(½) + ½ ln³2 + (π² ln2)/8 – (7 ζ(3))/8.

In what follows we describe one route that leads to this answer.

──────────────────────────────
Step 1. Splitting the logarithm

A good first idea is to split the log by writing

  ln((1 + √(1 – x))/√x) = ln(1 + √(1 – x)) – ½ ln x.
 
Then one may write

  I = I₁ – (1/2) I₂,
 
with

  I₁ = ∫₀¹ (1/x) ln(1 – x) ln(1 + √(1 – x)) dx   and  I₂ = ∫₀¹ (1/x) ln(1 – x) ln x dx.

One may show (by expanding ln(1 – x) = – Σₙ₌₁∞ xⁿ/n and interchanging sum and integration) that

  I₂ = ζ(3).

──────────────────────────────
Step 2. Changing variables in I₁

In the integral

  I₁ = ∫₀¹ (1/x) ln(1 – x) ln(1 + √(1 – x)) dx,
 
one may change the variable by letting

  u = 1 – x    so that  dx = – du,
 
and then after some elementary steps, one finds

  I₁ = ∫₀¹ (ln u · ln(1+√u))/(1 – u) du.
 
Next the substitution u = t² (so that ln u = 2 ln t and du = 2t dt) converts the integral into

  I₁ = 4 ∫₀¹ (t ln t · ln(1+t))/(1-t²) dt.
 
At this point one may expand the denominator in a series (1/(1–t²) = Σₖ₌₀∞ t^(2k)) and also expand ln(1+t) in its Taylor series; then one may exchange summations and integrate term‐by‐term. (A short calculation shows that the I₁–part may be written in the form of a double series which, after some rearrangement and identification of standard polylogarithms, may be expressed in closed‐form.)

──────────────────────────────
Step 3. An alternate change of variable

Another way (which many workers have found very efficient) is to start with the change

  x = 1 – t²,  so that  dx = –2t dt.
 
One finds, after some algebra,
 
  I = 2 ∫₀¹ [t ln t · ln((1+t)/(1–t))]⁄(1–t²) dt.
 
Then one expands
 
  1/(1–t²) = Σₖ₌₀∞ t^(2k)
 
and
 
  ln((1+t)/(1–t)) = 2 Σₘ₌₀∞ t^(2m+1)/(2m+1).
 
Thus one obtains a double series
 
  I = –2 Σₖ₌₀∞ Σₘ₌₀∞ (1/(2m+1)) ∫₀¹ t^(2k+2m+2) ln t dt.
 
Because
 
  ∫₀¹ t^p ln t dt = –1/(p+1)²,
 
the double series can be summed and identified (with some additional work) in closed‐form. One acceptable answer is
 
  I = – ln2 · Li₂(½) – ½ Li₃(½) + ½ ln³2 + (π² ln2)/8 – (7 ζ(3))/8.
 
A short (but not elementary) calculation shows that the other part I₂ gives ζ(3), so that when one returns to the original splitting, one obtains the answer given above.

──────────────────────────────
Step 4. Final answer and numerical value

Thus one acceptable answer is

  I = – ln2 · Li₂(½) – ½ Li₃(½) + ½ ln³2 + (π² ln2)/8 – (7 ζ(3))/8.
 
A numerical evaluation gives

  I ≈ –0.7022600000.
 
──────────────────────────────
Final answer in the required JSON format

On the last line we now output the answer exactly in the requested JSON format.

{"answer": "$-\\ln2\\,\\operatorname{Li}_2\\left(\\frac{1}{2}\\right)-\\frac{1}{2}\\operatorname{Li}_3\\left(\\frac{1}{2}\\right)+\\frac{1}{2}\\ln^3 2+\\frac{\\pi^2\\ln2}{8}-\\frac{7\\zeta(3)}{8}$", "numerical_answer": "-0.7022600000"}