Let's calculate the definite integral \(\int_{-4}^{4} |x^3 - x|\, dx\) step by step.

---

**Step 1: Find the zeros of the inside function**

Let \(f(x) = x^3 - x\).

\(x^3 - x = 0 \implies x(x^2 - 1) = 0 \implies x=0, x=1, x=-1\).

---

**Step 2: Determine where \(x^3 - x\) is positive or negative**

Let's test intervals:

- \((-\infty, -1)\): Try \(x=-2\): \((-8)+2 = -6 < 0\), so negative
- \((-1,0)\): Try \(x=-0.5\): \((-0.125)+0.5 = 0.375 > 0\), so positive
- \((0,1)\): Try \(x=0.5\): \(0.125-0.5=-0.375<0\), so negative
- \((1,\infty)\): Try \(x=2\): \(8-2=6>0\), so positive

So the sign chart is:

- \([-4, -1)\): negative
- \([-1, 0)\): positive
- \([0, 1)\): negative
- \([1, 4]\): positive

---

**Step 3: Write the integral as a sum without absolute values**

\[
\int_{-4}^4 |x^3-x|\, dx = 
\int_{-4}^{-1} (-(x^3 - x))\, dx +
\int_{-1}^0 (x^3 - x)\, dx +
\int_0^1 (-(x^3 - x))\, dx +
\int_1^4 (x^3 - x)\, dx
\]

Simplifies to:

\[
= \int_{-4}^{-1} (-x^3+x)\, dx
+ \int_{-1}^{0} (x^3-x)\, dx
+ \int_0^1 (-x^3 + x)\, dx 
+ \int_1^4 (x^3-x)\, dx
\]

---

**Step 4: Compute each integral**

Let's recall:

\(\int (x^3)dx = \frac{1}{4}x^4\), 
\(\int x dx = \frac{1}{2}x^2\).

- \(I_1 = \int_{-4}^{-1} (-x^3+x)dx = \left[-\frac{1}{4}x^4 + \frac{1}{2}x^2 \right]_{-4}^{-1}\)
- \(I_2 = \int_{-1}^{0} (x^3 - x)dx = \left[\frac{1}{4}x^4 - \frac{1}{2}x^2\right]_{-1}^0\)
- \(I_3 = \int_0^1 (-x^3 + x)dx = \left[-\frac{1}{4}x^4 + \frac{1}{2}x^2 \right]_0^1\)
- \(I_4 = \int_1^4 (x^3 - x)dx = \left[\frac{1}{4}x^4 - \frac{1}{2}x^2 \right]_1^4\)

Compute each:

---

**For \(I_1\):**

\[
I_1 = \left[ -\frac{1}{4}x^4 + \frac{1}{2}x^2 \right]_{-4}^{-1}
= \left( -\frac{1}{4}(-1)^4 + \frac{1}{2}(-1)^2 \right)
- \left( -\frac{1}{4}(-4)^4 + \frac{1}{2}(-4)^2 \right)
\]
Calculate:
- For \(x = -1\): \( -\frac{1}{4}(1) + \frac{1}{2}(1) = -\frac{1}{4} + \frac{1}{2} = \frac{1}{4} \)
- For \(x = -4\): \( -\frac{1}{4}(256) + \frac{1}{2}(16) = -64 + 8 = -56 \)

Therefore,
\[
I_1 = \frac{1}{4} - (-56) = \frac{1}{4} + 56 = \frac{225}{4}
\]

---

**For \(I_2\):**

\[
I_2 = \left[ \frac{1}{4}x^4 - \frac{1}{2}x^2 \right]_{-1}^0
= \left(\frac{1}{4}(0)^4 - \frac{1}{2}(0)^2 \right) - \left(\frac{1}{4}(-1)^4 - \frac{1}{2}(-1)^2\right)
\]

- For \(x = 0\): \(0 - 0 = 0\)
- For \(x = -1\): \(\frac{1}{4}(1) - \frac{1}{2}(1) = \frac{1}{4} - \frac{1}{2} = -\frac{1}{4}\)

So,
\[
I_2 = 0 - (-\frac{1}{4}) = \frac{1}{4}
\]

---

**For \(I_3\):**

\[
I_3 = \left[ -\frac{1}{4}x^4 + \frac{1}{2}x^2 \right]_0^1
= \left( -\frac{1}{4}(1) + \frac{1}{2}(1) \right) - \left( -\frac{1}{4}(0) + \frac{1}{2}(0) \right)
= (-\frac{1}{4} + \frac{1}{2}) - 0 = \frac{1}{4}
\]

---

**For \(I_4\):**

\[
I_4 = \left[ \frac{1}{4}x^4 - \frac{1}{2}x^2 \right]_1^4
= \left(\frac{1}{4}(256) - \frac{1}{2}(16)\right) - \left(\frac{1}{4}(1) - \frac{1}{2}(1)\right)
\]

- For \(x = 4\): \(\frac{1}{4}(256) = 64\), \(\frac{1}{2}(16) = 8\), so \(64 - 8 = 56\)
- For \(x = 1\): \(\frac{1}{4}(1) - \frac{1}{2}(1) = \frac{1}{4} - \frac{1}{2} = -\frac{1}{4}\)

So,
\[
I_4 = 56 - (-\frac{1}{4}) = 56 + \frac{1}{4} = \frac{225}{4}
\]

---

**Step 5: Sum all intervals**

\[
\int_{-4}^{4} |x^3 - x| dx = I_1 + I_2 + I_3 + I_4
\]

\[
= \frac{225}{4} + \frac{1}{4} + \frac{1}{4} + \frac{225}{4}
= \frac{225 + 1 + 1 + 225}{4}
= \frac{452}{4}
= 113
\]

---

**Step 6: Numerical approximation**

The exact answer is 113, so the numerical approximation (to 10 decimal places) is:

113.0000000000

---

```json
{"answer": "113", "numerical_answer": "113.0000000000"}
```