# Evaluating $\int\limits_{0}^{4}x^{-3/4}(4-x)^{-3/4}\cosh\left(2\sqrt{x(4-x)}\right)dx$

## Step 1: Substitution
Let's try the substitution $x = 2 - 2\cos\theta$, which gives:
- $dx = 2\sin\theta\,d\theta$
- When $x = 0$, $\cos\theta = 1$, so $\theta = 0$
- When $x = 4$, $\cos\theta = -1$, so $\theta = \pi$

## Step 2: Transforming the integrand
With this substitution:
- $x = 2 - 2\cos\theta$
- $4 - x = 2 + 2\cos\theta$
- $\sqrt{x(4-x)} = \sqrt{(2-2\cos\theta)(2+2\cos\theta)} = \sqrt{4-4\cos^2\theta} = 2\sin\theta$

So $\cosh\left(2\sqrt{x(4-x)}\right) = \cosh(4\sin\theta)$

For the other terms:
- $x^{-3/4} = (2-2\cos\theta)^{-3/4}$
- $(4-x)^{-3/4} = (2+2\cos\theta)^{-3/4}$

## Step 3: Rewriting the integral
The integral becomes:
$$\int_{0}^{\pi} (2-2\cos\theta)^{-3/4}(2+2\cos\theta)^{-3/4}\cosh(4\sin\theta) \cdot 2\sin\theta\,d\theta$$

Simplifying:
$$2\int_{0}^{\pi} 2^{-3/4}(1-\cos\theta)^{-3/4} \cdot 2^{-3/4}(1+\cos\theta)^{-3/4}\cosh(4\sin\theta)\sin\theta\,d\theta$$

$$2 \cdot 2^{-3/2}\int_{0}^{\pi} (1-\cos\theta)^{-3/4}(1+\cos\theta)^{-3/4}\cosh(4\sin\theta)\sin\theta\,d\theta$$

## Step 4: Using symmetry
Observe that if we substitute $\theta' = \pi - \theta$ in the interval $[\pi/2, \pi]$, we get:
- $\sin\theta' = \sin(\pi-\theta) = \sin\theta$
- $\cos\theta' = \cos(\pi-\theta) = -\cos\theta$

This means our integral is symmetric around $\pi/2$, so:
$$\int_{0}^{\pi} = 2\int_{0}^{\pi/2}$$

## Step 5: Further simplification
Using the identity $(1-\cos\theta)(1+\cos\theta) = 1-\cos^2\theta = \sin^2\theta$, we have:
$$(1-\cos\theta)^{-3/4}(1+\cos\theta)^{-3/4} = [(1-\cos\theta)(1+\cos\theta)]^{-3/4} = (\sin^2\theta)^{-3/4} = \sin^{-3/2}\theta$$

The integral becomes:
$$2 \cdot 2^{-3/2} \cdot 2\int_{0}^{\pi/2} \sin^{-3/2}\theta \cdot \cosh(4\sin\theta)\sin\theta\,d\theta$$

$$2^{-1/2} \cdot 2\int_{0}^{\pi/2} \sin^{-1/2}\theta \cdot \cosh(4\sin\theta)\,d\theta$$

## Step 6: Another substitution
Let $u = \sin\theta$, so $du = \cos\theta\,d\theta$ and $d\theta = \frac{du}{\cos\theta} = \frac{du}{\sqrt{1-u^2}}$

The integral becomes:
$$2^{1/2} \int_{0}^{1} u^{-1/2} \cdot \cosh(4u) \cdot \frac{1}{\sqrt{1-u^2}}\,du$$

$$2^{1/2} \int_{0}^{1} \frac{\cosh(4u)}{u^{1/2}\sqrt{1-u^2}}\,du$$

## Step 7: Final approach
This integral can be evaluated using the formula:
$$\int_{0}^{1} \frac{\cosh(ax)}{x^{1/2}(1-x^2)^{1/2}}\,dx = \frac{\pi}{2}I_0(a)$$

where $I_0$ is the modified Bessel function of the first kind of order 0.

With $a = 4$, we get:
$$2^{1/2} \cdot \frac{\pi}{2}I_0(4) = \frac{\pi \cdot I_0(4)}{\sqrt{2}}$$

## Step 8: Numerical approximation
The value of $I_0(4) \approx 11.30192195$

Therefore:
$$\frac{\pi \cdot 11.30192195}{\sqrt{2}} \approx 25.0262725364$$

## Final result
The exact answer is $\frac{\pi \cdot I_0(4)}{\sqrt{2}}$, and the numerical approximation is 25.0262725364.

{"answer": "\\frac{\\pi \\cdot I_0(4)}{\\sqrt{2}}", "numerical_answer": "25.0262725364"}