

To solve the definite integral \(\int_0^1 (x-1)^2(x+1)^2(x^2+1)^2(x^4+1)^2 \, dx\), we start by simplifying the integrand using algebraic identities.

### Step 1: Simplify the integrand
Notice that the integrand can be simplified using the difference of squares repeatedly:
- First, \((x-1)^2(x+1)^2 = [(x-1)(x+1)]^2 = (x^2 - 1)^2\).
- Next, \((x^2 - 1)^2(x^2 + 1)^2 = [(x^2 - 1)(x^2 + 1)]^2 = (x^4 - 1)^2\).
- Then, \((x^4 - 1)^2(x^4 + 1)^2 = [(x^4 - 1)(x^4 + 1)]^2 = (x^8 - 1)^2\).

Thus, the integrand simplifies to \((x^8 - 1)^2\).

### Step 2: Expand the simplified integrand
Expanding \((x^8 - 1)^2\) gives:
\[
(x^8 - 1)^2 = x^{16} - 2x^8 + 1
\]

### Step 3: Integrate term by term
We now integrate the expanded polynomial from \(0\) to \(1\):
\[
\int_0^1 (x^{16} - 2x^8 + 1) \, dx
\]

Integrate each term separately:
- \(\int_0^1 x^{16} \, dx = \left[ \frac{x^{17}}{17} \right]_0^1 = \frac{1}{17}\)
- \(\int_0^1 -2x^8 \, dx = -2 \left[ \frac{x^9}{9} \right]_0^1 = -2 \cdot \frac{1}{9} = -\frac{2}{9}\)
- \(\int_0^1 1 \, dx = \left[ x \right]_0^1 = 1\)

### Step 4: Combine the results
Adding these results together:
\[
\frac{1}{17} - \frac{2}{9} + 1
\]

To combine the fractions, use a common denominator (153):
\[
\frac{1}{17} = \frac{9}{153}, \quad \frac{2}{9} = \frac{34}{153}, \quad 1 = \frac{153}{153}
\]
\[
\frac{9}{153} - \frac{34}{153} + \frac{153}{153} = \frac{9 - 34 + 153}{153} = \frac{128}{153}
\]

### Step 5: Numerical approximation
The exact value is \(\frac{128}{153}\). Numerically, this is approximately \(0.8366013072\) (rounded to 10 decimal places).

{"answer": "\(\frac{128}{153}\)", "numerical_answer": "0.8366013072"}