Let's proceed step by step.

Let  
\[ I = \int_{420}^{1672} \frac{\sqrt{\ln(2023-x)}}{\sqrt{\ln(2023-x)}+\sqrt{\ln(x-69)}} \, dx \]

#### **Step 1: Symmetry and Substitution**

Let us try the substitution:  
Let \( u = 2023 - x \).

- When \( x = 420, u = 2023 - 420 = 1603 \).
- When \( x = 1672, u = 2023 - 1672 = 351 \).

Also,
- \( dx = -du \)
- \( \ln(2023-x) = \ln u \)
- \( x-69 = 2023-u-69 = (2023-69)-u = 1954-u \)
- \( \ln(x-69) = \ln(1954-u) \)

So, rewrite the integral (reverse the limits due to \( dx = - du \)):

\[
I = \int_{u=1603}^{u=351} \frac{\sqrt{\ln u}}{\sqrt{\ln u} + \sqrt{\ln(1954-u)}} (-du)
\]
\[
= \int_{u=351}^{1603} \frac{\sqrt{\ln u}}{\sqrt{\ln u} + \sqrt{\ln(1954-u)}} du
\]

Now, let's compare that to the original integral.

If we make another substitution in the original variable:  
Let \( y = x \), so:

\[
I = \int_{x=420}^{1672} \frac{\sqrt{\ln(2023-x)}}{\sqrt{\ln(2023-x)}+\sqrt{\ln(x-69)}} dx
\]

But notice something interesting with the bounds:  
- \( 420 + 1603 = 2023 \)
- \( 1672 + 351 = 2023 \)

So generally, for \( x \) in \( [420, 1672] \), \( (2023 - x) \) is in \( [351, 1603] \).

#### **Sum with Complement Integral**

Letâ€™s compute
\[
I' = \int_{x=420}^{1672} \frac{\sqrt{\ln(x-69)}}{\sqrt{\ln(2023-x)}+\sqrt{\ln(x-69)}} dx
\]

Notice \( I + I' \):
\[
I + I' = \int_{420}^{1672} \frac{\sqrt{\ln(2023-x)} + \sqrt{\ln(x-69)}}{\sqrt{\ln(2023-x)} + \sqrt{\ln(x-69)}} dx = \int_{420}^{1672} 1\,dx = 1672 - 420 = 1252
\]

That is,
\[
I + I' = 1252
\]

But, by the substitution above, we saw the region exchanged the roles of the two square roots upon \( x \mapsto 2023 - x \). Therefore, by the substitution, \( I' = I \) (because the bounds and function are symmetric under the swap).

Therefore,
\[
2I = 1252 \implies I = \frac{1252}{2} = 626
\]

---

#### **Step 2: Final Results**

**Exact Value:**
\[
\boxed{626}
\]

**Numerical Value:**
\[
626.0000000000
\]

---

```json
{"answer": "626", "numerical_answer": "626.0000000000"}
```