Let's carefully compute the integral:
\[
I = \int_0^1 \left\lfloor \cos\left( \frac{\pi}{x} \right) \right\rfloor\, dx
\]

### Step 1: Analyze the function

\(\cos(\frac{\pi}{x})\) is continuous on \((0,1]\). Because \(\cos\) oscillates between \(-1\) and \(1\), but the argument \(\frac{\pi}{x}\) tends to infinity as \(x \to 0^+\).

The floor function \(\left\lfloor \cos(\frac{\pi}{x}) \right\rfloor\) will only take integer values \(-1\) and \(0\) on \((0, 1]\), because for all \(x\) in \((0,1]\), \(\cos(\frac{\pi}{x})\) is always between \(-1\) and \(1\), but never actually reaches \(1\), so the floor is at most 0.

So, the integrand is either \(-1\) or \(0\):
- It equals 0 where \(\cos(\frac{\pi}{x}) \in [0,1)\),
- It equals \(-1\) where \(\cos(\frac{\pi}{x}) \in [-1, 0)\).

So, the question is for which \(x\) in \((0,1]\) do we have \(\cos(\frac{\pi}{x}) < 0\)? This happens when the argument is in odd multiples of \(\pi\).

\[
\cos\theta < 0 \iff \theta \in \left( \frac{\pi}{2} + k\pi, \frac{3\pi}{2} + k\pi \right),\, k \in \mathbb{Z}
\]

Let \(y = 1/x\), so as \(x\) goes from 0 to 1, \(y\) goes from \(\infty\) to 1.

\[
\cos(\pi / x) < 0 \iff \frac{\pi}{x} \in \left( (2k+1)\frac{\pi}{2}, (2k+3)\frac{\pi}{2} \right), \qquad k = 0,1,2,\dots
\]
So,
\[
(2k+1)\frac{\pi}{2} < \frac{\pi}{x} < (2k+3)\frac{\pi}{2}
\implies
\frac{2}{2k+3} < x < \frac{2}{2k+1}
\]

But we have to intersect these intervals with \((0,1]\).

Define:
\[
A_k = \left( \frac{2}{2k+3}, \frac{2}{2k+1} \right) \cap (0,1]
\]

Now, for which \(k\) are these intervals contained in \((0,1]\)?
- For the right endpoint, \(\frac{2}{2k+1}>1 \implies 2k+1 < 2 \implies k=0\) (since for \(k=1\), \(2k+1=3\), \(2/3<1\)).
- The left endpoints: \(\frac{2}{2k+3}\): as \(k\) increases, this gets smaller.

So for \(k=0\): \((2/3,2/1) = (2/3,2)\), intersected with \((0,1]\) gives \((2/3,1]\).

For \(k=1\): \((2/5,2/3)\), both less than 1, so included.

Similarly for \(k=2\): \((2/7,2/5)\), both <1.

Continue until \(\frac{2}{2k+1} < 0\), which cannot happen for positive \(k\). But for all \(k\), the interval is inside \((0,1]\) when \(\frac{2}{2k+1} \leq 1\), i.e. \(2k+1 \geq 2\), \(k \geq 1/2\). But let's check explicitly:

- For \(k=0\): \((2/3,1]\)
- For \(k=1\): \((2/5,2/3)\)
- For \(k=2\): \((2/7,2/5)\)
- etc.

So the set where the integrand is \(-1\) is:
\[
\bigcup_{k=0}^\infty \left( \max\left(0,\frac{2}{2k+3}\right), \min\left(1, \frac{2}{2k+1}\right) \right)
\]

We need all intervals inside \((0,1]\), i.e., as \(k \to \infty\), their endpoints approach zero.

### Step 2: Express the integral as a sum

On each interval, the function is \(-1\), and on the complement, it's 0.

So,
\[
I = \sum_{k=0}^\infty \left( \min\left(1, \frac{2}{2k+1}\right) - \max\left(0, \frac{2}{2k+3}\right) \right)
\]

But for \(k=0\), \(\frac{2}{2k+1}\) is 2, so \(\min(1,2)=1\),
and \(\frac{2}{2k+3} = 2/3 > 0\), so the interval is \((2/3,1]\) length \(1-2/3=1/3\).

For \(k\geq 1\):
- \(\frac{2}{2k+1} < 1\), so \(\min\) is just \(\frac{2}{2k+1}\),
- and \(\frac{2}{2k+3} > 0\), so \(\max\) is \(\frac{2}{2k+3}\).

Thus for \(k=0\): interval \((2/3,1]\) of length \(1-2/3 = 1/3\)

For \(k\geq 1\): interval \((2/(2k+3), 2/(2k+1))\) length:
\[
\frac{2}{2k+1} - \frac{2}{2k+3} = 2\left( \frac{1}{2k+1} - \frac{1}{2k+3} \right)
= 2 \cdot \frac{(2k+3)-(2k+1)}{(2k+1)(2k+3)}
= 2 \cdot \frac{2}{(2k+1)(2k+3)}
= \frac{4}{(2k+1)(2k+3)}
\]

Therefore,
\[
I = -\left[ \frac{1}{3} + \sum_{k=1}^\infty \frac{4}{(2k+1)(2k+3)} \right]
\]

### Step 3: Simplify the series

Let's try to write \(\frac{4}{(2k+1)(2k+3)}\) in a telescoping form:

\[
\frac{4}{(2k+1)(2k+3)} = A \left(\frac{1}{2k+1}-\frac{1}{2k+3}\right)
\]
Solving for \(A\):

\[
A \left( \frac{1}{2k+1} - \frac{1}{2k+3} \right)
= A \cdot \frac{2}{(2k+1)(2k+3)}
\implies A = 2
\]
So,
\[
\frac{4}{(2k+1)(2k+3)} = 2 \left( \frac{1}{2k+1} - \frac{1}{2k+3} \right)
\]
Therefore,
\[
I = -\frac{1}{3} - \sum_{k=1}^\infty 2 \left( \frac{1}{2k+1} - \frac{1}{2k+3} \right)
\]

This sum telescopes if we sum from \(k=1\) to \(n\):

\[
S_n = 2 \sum_{k=1}^n \left( \frac{1}{2k+1} - \frac{1}{2k+3} \right)
= 2 \left( \left(\frac{1}{3} - \frac{1}{5}\right) + \left(\frac{1}{5} - \frac{1}{7}\right) + \dots + \left( \frac{1}{2n+1} - \frac{1}{2n+3}\right) \right)
\]
This collapses to
\[
2 \left(\frac{1}{3} - \frac{1}{2n+3}\right)
\]
Therefore as \(n \to \infty\), \(\frac{1}{2n+3}\to 0\):

\[
\sum_{k=1}^\infty 2 \left( \frac{1}{2k+1} - \frac{1}{2k+3} \right) = 2\left(\frac{1}{3}\right) = \frac{2}{3}
\]

So, finally,
\[
I = -\frac{1}{3} - \frac{2}{3} = -1
\]

### Step 4: Numerical approximation

Final answer is \(-1\), which rounded to 10 decimal places is
\(-1.0000000000\)

---

```json
{"answer": "-1", "numerical_answer": "-1.0000000000"}
```