<think>
Okay, let's tackle this integral step by step. The integral given is ∫₀² x^(1.0 - 3/2) (2.0 - x)^(1.0 - 1/2) [1 - 0.5x(2.0 - x)]^(-1.0) dx. First, I need to simplify the exponents and the integrand to see if it matches a known form or if a substitution can be applied.

Starting with the exponents: 1.0 - 3/2 is equal to -1/2, and 1.0 - 1/2 is 1/2. So the integral becomes ∫₀² x^(-1/2) (2 - x)^(1/2) [1 - 0.5x(2 - x)]^(-1) dx. Let me write that more neatly: ∫₀² x^(-1/2) (2 - x)^(1/2) / [1 - 0.5x(2 - x)] dx.

Next, let's simplify the denominator. The term 0.5x(2 - x) can be expanded. Let's compute that: 0.5x(2 - x) = x - 0.5x². So the denominator becomes 1 - x + 0.5x². Hmm, that's a quadratic expression. Let me check if it can be factored or rewritten in a more manageable form. Let's see: 0.5x² - x + 1. Maybe completing the square? Let's factor out 0.5 first: 0.5(x² - 2x) + 1. Completing the square inside the parentheses: x² - 2x + 1 - 1 = (x - 1)^2 - 1. So, 0.5[(x - 1)^2 - 1] + 1 = 0.5(x - 1)^2 - 0.5 + 1 = 0.5(x - 1)^2 + 0.5. So the denominator is 0.5[(x - 1)^2 + 1]. Therefore, 1 - 0.5x(2 - x) = 0.5[(x - 1)^2 + 1]. Therefore, the integrand becomes [0.5((x - 1)^2 + 1)]^(-1) = 2 / [(x - 1)^2 + 1]. 

So putting it all together, the integral is ∫₀² x^(-1/2) (2 - x)^(1/2) * 2 / [(x - 1)^2 + 1] dx. Let me write that as 2 ∫₀² [x^(-1/2) (2 - x)^(1/2)] / [(x - 1)^2 + 1] dx. 

Now, looking at the numerator inside the integral: x^(-1/2) (2 - x)^(1/2) can be written as sqrt((2 - x)/x). So the integrand becomes 2 * sqrt((2 - x)/x) / [(x - 1)^2 + 1]. Hmm, this seems a bit complicated. Maybe a substitution would help here. Let's consider substituting t = x - 1 to center the integral around zero. Let t = x - 1, so x = t + 1, and when x=0, t=-1; x=2, t=1. Then dx = dt. The integral becomes 2 ∫_{-1}^1 sqrt((2 - (t + 1))/(t + 1)) / [t² + 1] dt. Simplifying the numerator inside the sqrt: (2 - t -1)/(t + 1) = (1 - t)/(1 + t). So sqrt((1 - t)/(1 + t)). Therefore, the integral is 2 ∫_{-1}^1 sqrt((1 - t)/(1 + t)) / (t² + 1) dt. 

This looks like it might be related to a standard integral or perhaps a trigonometric substitution. The term sqrt((1 - t)/(1 + t)) suggests using a substitution like t = cosθ, but let's see. Let me try substituting u = sqrt((1 - t)/(1 + t)). Let's set u = sqrt((1 - t)/(1 + t)). Then u² = (1 - t)/(1 + t). Solving for t: u²(1 + t) = 1 - t → u² + u² t = 1 - t → t(u² + 1) = 1 - u² → t = (1 - u²)/(1 + u²). Then dt/du = [ -2u(1 + u²) - (1 - u²)(2u) ] / (1 + u²)^2. Let me compute that: numerator is -2u(1 + u²) - 2u(1 - u²) = -2u - 2u³ - 2u + 2u³ = -4u. So dt = -4u / (1 + u²)^2 du. 

But when t = -1, u = sqrt((1 - (-1))/(1 + (-1))) = sqrt(2/0), which is undefined. Hmm, that's a problem. Maybe this substitution isn't the best approach. Alternatively, perhaps a trigonometric substitution. Let's consider t = sinθ. Wait, but the denominator is t² + 1, which is 1 + t². If we set t = tanθ, then t² + 1 = sec²θ, which might simplify. Let's try that. Let t = tanθ, so dt = sec²θ dθ. Then the integral becomes 2 ∫_{θ=-π/4}^{θ=π/4} sqrt((1 - tanθ)/(1 + tanθ)) * sec²θ / (tan²θ + 1) dθ. But tan²θ + 1 is sec²θ, so the denominator becomes sec²θ, which cancels with the sec²θ in the numerator. So the integral simplifies to 2 ∫_{-π/4}^{π/4} sqrt((1 - tanθ)/(1 + tanθ)) dθ. 

Now, let's simplify the sqrt term. Let's note that (1 - tanθ)/(1 + tanθ) can be written as [ (cosθ - sinθ)/cosθ ] / [ (cosθ + sinθ)/cosθ ] = (cosθ - sinθ)/(cosθ + sinθ). So sqrt of that is sqrt( (cosθ - sinθ)/(cosθ + sinθ) ). Let's multiply numerator and denominator inside the sqrt by (cosθ - sinθ): sqrt( (cosθ - sinθ)^2 / (cos²θ - sin²θ) ). Wait, but that might complicate things. Alternatively, note that (cosθ - sinθ)/(cosθ + sinθ) = [1 - tanθ]/[1 + tanθ], which is the same as before. Maybe we can write this as tan(π/4 - θ). Because tan(π/4 - θ) = (1 - tanθ)/(1 + tanθ). Therefore, sqrt(tan(π/4 - θ)). So the integrand becomes sqrt(tan(π/4 - θ)). 

So the integral is 2 ∫_{-π/4}^{π/4} sqrt(tan(π/4 - θ)) dθ. Let's make a substitution here. Let φ = π/4 - θ. Then when θ = -π/4, φ = π/4 - (-π/4) = π/2; when θ = π/4, φ = π/4 - π/4 = 0. So the limits switch from π/2 to 0, and dφ = -dθ. Therefore, the integral becomes 2 ∫_{π/2}^0 sqrt(tanφ) (-dφ) = 2 ∫₀^{π/2} sqrt(tanφ) dφ. 

So now we have 2 times the integral of sqrt(tanφ) from 0 to π/2. This is a standard integral. Let me recall that ∫₀^{π/2} tan^nφ dφ = π/(2 cos(nπ/2)) for -1 < n < 1. But here we have sqrt(tanφ) = tan^{1/2}φ. So n = 1/2. Then the integral would be π/(2 cos(π/4)) = π/(2*(√2/2)) = π/√2. Therefore, ∫₀^{π/2} sqrt(tanφ) dφ = π/√2. Therefore, multiplying by 2, the original integral becomes 2*(π/√2) = √2 π. 

Wait, but let me verify this result because sometimes these standard integrals can be tricky. Alternatively, let's compute ∫₀^{π/2} sqrt(tanφ) dφ. Let me use substitution. Let u = sinφ, then du = cosφ dφ. But maybe a better substitution is to set t = tanφ. Let t = tanφ, so φ from 0 to π/2 corresponds to t from 0 to ∞. Then dφ = dt/(1 + t²). The integral becomes ∫₀^∞ sqrt(t) * (1/(1 + t²)) dt. So ∫₀^∞ t^{1/2}/(1 + t²) dt. This is a standard Beta function integral. Recall that ∫₀^∞ t^{k - 1}/(1 + t)^{m} dt = B(k, m - k) for m > k > 0. But here it's t², not t. Let me make substitution. Let u = t², then t = u^{1/2}, dt = (1/2)u^{-1/2} du. Then the integral becomes ∫₀^∞ (u^{1/4})/(1 + u) * (1/2)u^{-1/2} du = (1/2) ∫₀^∞ u^{-1/4}/(1 + u) du. This is similar to the Beta function. The integral ∫₀^∞ u^{s - 1}/(1 + u) du = π/sin(πs) for 0 < s < 1. Here, s = 3/4 (since s - 1 = -1/4 → s = 3/4). Therefore, the integral is (1/2) * π/sin(3π/4) = (1/2) * π/(√2/2) = (1/2) * π * 2/√2 = π/√2. So yes, the integral ∫₀^{π/2} sqrt(tanφ) dφ = π/√2. Therefore, multiplying by 2 gives √2 π. 

Therefore, the original integral evaluates to √2 π. Let me check the steps again to make sure there are no mistakes. Starting from the original integral, substitution t = x - 1, transformed into an integral from -1 to 1, then substitution t = tanθ leading to integrating sqrt(tanφ) from 0 to π/2, which gives π/√2, multiplied by 2 gives √2 π. That seems correct. 

Now, the numerical approximation. The exact answer is √2 π. Let's compute that. √2 is approximately 1.41421356237, and π is approximately 3.14159265359. Multiplying them: 1.41421356237 * 3.14159265359 ≈ 4.442882908158366. Rounded to 10 decimal places, that's 4.4428829082. 

Wait, let me compute it more accurately. Let's use more decimal places for √2 and π. √2 ≈ 1.4142135623730950488016887242097, π ≈ 3.1415926535897932384626433832795. Multiplying these: 1.4142135623730950488016887242097 * 3.1415926535897932384626433832795. Let's compute this step by step. 

First, 1.414213562373095 * 3.141592653589793 ≈ 

Let me compute 1.4142 * 3.141592653589793:

1.4142 * 3 = 4.2426

1.4142 * 0.141592653589793 ≈ 1.4142 * 0.1415926536 ≈ 

0.1415926536 * 1 = 0.1415926536

0.1415926536 * 0.4 = 0.05663706144

0.1415926536 * 0.1 = 0.01415926536

0.1415926536 * 0.004 = 0.0005663706144

Adding up: 0.1415926536 + 0.05663706144 = 0.19822971504 + 0.01415926536 = 0.2123889804 + 0.0005663706144 ≈ 0.212955351. So total is approximately 4.2426 + 0.212955351 ≈ 4.455555351. But this is a rough estimate. However, using a calculator-like approach, √2 * π ≈ 4.442882908158366. Rounded to 10 decimal places, that's 4.4428829082. 

Therefore, the exact answer is √2 π, and the numerical approximation is approximately 4.4428829082.
</think>

{"answer": "\\sqrt{2} \\pi", "numerical_answer": "4.4428829082"}