Let’s compute the integral:
\[
I = \int_0^{\frac{\pi}{4}}\tan^{-1}\left(\frac{1+\tan(x)}{\sqrt{2}}\right)\mathrm{d}x
\]

## **Step 1: Substitution & Simplification**

Let’s try the substitution \( x \mapsto \frac{\pi}{4} - x \).

- When \( x = 0 \Rightarrow y = \frac{\pi}{4} \)
- When \( x = \frac{\pi}{4} \Rightarrow y = 0 \)

So,
\[
I = \int_0^{\frac{\pi}{4}} \tan^{-1}\left(\frac{1+\tan x}{\sqrt{2}}\right) dx
\]
Now set \( y = \frac{\pi}{4} - x \), \( dx = -dy \), limits flip, giving:
\[
I = \int_{\frac{\pi}{4}}^{0} \tan^{-1}\left(\frac{1+\tan\left(\frac{\pi}{4} - y\right)}{\sqrt{2}}\right) (-dy) = \int_{0}^{\frac{\pi}{4}} \tan^{-1}\left(\frac{1+\tan\left(\frac{\pi}{4} - y\right)}{\sqrt{2}}\right)\,dy
\]

Evaluate \(\tan\left(\frac{\pi}{4} - y\right)\):

\[
\tan\left(\frac{\pi}{4} - y\right) = \frac{1-\tan y}{1+\tan y}
\]

Thus,

\[
I = \int_{0}^{\frac{\pi}{4}} \tan^{-1}\left(\frac{1 + \frac{1-\tan y}{1+\tan y}}{\sqrt{2}}\right) dy
\]

Simplify numerator:

\[
1 + \frac{1-\tan y}{1+\tan y} = \frac{(1+\tan y) + (1-\tan y)}{1+\tan y} = \frac{2}{1+\tan y}
\]

So the inner argument becomes:

\[
\tan^{-1}\left(\frac{2}{\sqrt{2}(1+\tan y)}\right) = \tan^{-1}\left( \frac{\sqrt{2}}{1+\tan y} \right )
\]

So,
\[
I = \int_0^{\frac{\pi}{4}}\tan^{-1}\left(\frac{\sqrt{2}}{1+\tan x}\right)\mathrm{d}x
\]

## **Step 2: Add the Integral To Itself**

Let’s denote the original integrand as \( f(x) = \tan^{-1}\left(\frac{1+\tan x}{\sqrt{2}}\right) \), and via substitution above, \( f_1(x) = \tan^{-1}\left(\frac{\sqrt{2}}{1+\tan x}\right) \).

Notice:

\[
I = \int_0^{\frac{\pi}{4}} f(x)\,dx = \int_0^{\frac{\pi}{4}} f_1(x)\,dx
\]

Therefore,

\[
2I = \int_0^{\frac{\pi}{4}} \left[ \tan^{-1}\left(\frac{1+\tan x}{\sqrt{2}}\right) + \tan^{-1}\left(\frac{\sqrt{2}}{1+\tan x}\right) \right] dx
\]

Now recall:

\[
\tan^{-1} a + \tan^{-1} b = \tan^{-1}\left( \frac{a+b}{1-ab} \right ), \quad \text{if } ab < 1
\]

(a quick check: for all \( x \) in the interval, both terms positive and the product less than 1)

Let’s compute:
\[
a = \frac{1+\tan x}{\sqrt{2}}, \ \ b = \frac{\sqrt{2}}{1+\tan x}
\]
So,
\[
a + b = \frac{1+\tan x}{\sqrt{2}} + \frac{\sqrt{2}}{1+\tan x} = \frac{(1+\tan x)^2 + 2}{\sqrt{2}(1+\tan x)}
\]
and
\[
a b = \frac{1+\tan x}{\sqrt{2}} \cdot \frac{\sqrt{2}}{1+\tan x} = 1
\]

So,
\[
\tan^{-1} a + \tan^{-1} b = \tan^{-1}\left( \infty \right ) = \frac{\pi}{2}
\]
(As denominator \(1-ab\) tends to zero: the sum jumps to \(\frac{\pi}{2}\).)

But let's double-check: For \(ab = 1\), then the sum is always \(\frac{\pi}{2}\) (since both are positive).

Therefore,

\[
2I = \int_0^{\frac{\pi}{4}} \frac{\pi}{2}\,dx = \frac{\pi}{2} \cdot \frac{\pi}{4} = \frac{\pi^2}{8}
\]
\[
I = \frac{\pi^2}{16}
\]

## **Step 3: Numerical Value**

\[
I = \frac{\pi^2}{16} \approx \frac{(3.1415926536)^2}{16} \approx \frac{9.8696044011}{16} \approx 0.6168502751
\]

## **Step 4: Final JSON Output**

```json
{"answer": "\\frac{\\pi^2}{16}", "numerical_answer": "0.6168502751"}
```