# Evaluating $\int_0^1(x-1)^2(x+1)^2(x^2+1)^2(x^4+1)^2\text{ dx}$

## Step 1: Expand the integrand

Let's denote the integrand as $f(x) = (x-1)^2(x+1)^2(x^2+1)^2(x^4+1)^2$

First, I'll expand each part:
- $(x-1)^2 = x^2 - 2x + 1$
- $(x+1)^2 = x^2 + 2x + 1$
- $(x^2+1)^2 = x^4 + 2x^2 + 1$
- $(x^4+1)^2 = x^8 + 2x^4 + 1$

Now I'll multiply these together step by step.

Let's start with $(x-1)^2(x+1)^2$:
$(x^2 - 2x + 1)(x^2 + 2x + 1) = x^4 + 2x^3 + x^2 - 2x^3 - 4x^2 - 2x + x^2 + 2x + 1$
$= x^4 - 2x^2 + 1 = (x^2)^2 - 2(x^2) + 1 = (x^2-1)^2$

So $(x-1)^2(x+1)^2 = (x^2-1)^2$

Now, multiply this by $(x^2+1)^2$:
$(x^2-1)^2(x^2+1)^2 = (x^4-2x^2+1)(x^4+2x^2+1)$
$= x^8 + 2x^6 + x^4 - 2x^6 - 4x^4 - 2x^2 + x^4 + 2x^2 + 1$
$= x^8 - 2x^4 + 1$
$= (x^4)^2 - 2(x^4) + 1 = (x^4-1)^2$

So $(x-1)^2(x+1)^2(x^2+1)^2 = (x^4-1)^2$

Finally, multiply by $(x^4+1)^2$:
$(x^4-1)^2(x^4+1)^2 = (x^8-2x^4+1)(x^8+2x^4+1)$
$= x^{16} + 2x^{12} + x^8 - 2x^{12} - 4x^8 - 2x^4 + x^8 + 2x^4 + 1$
$= x^{16} - 2x^8 + 1$
$= (x^8)^2 - 2(x^8) + 1 = (x^8-1)^2$

Therefore, our integrand simplifies to:
$f(x) = (x^8-1)^2 = x^{16} - 2x^8 + 1$

## Step 2: Integrate term by term

$\int_0^1 f(x) dx = \int_0^1 (x^{16} - 2x^8 + 1) dx$
$= \int_0^1 x^{16} dx - 2\int_0^1 x^8 dx + \int_0^1 1 dx$
$= \left[ \frac{x^{17}}{17} \right]_0^1 - 2\left[ \frac{x^9}{9} \right]_0^1 + \left[ x \right]_0^1$
$= \frac{1^{17}}{17} - \frac{0^{17}}{17} - 2\left(\frac{1^9}{9} - \frac{0^9}{9}\right) + (1 - 0)$
$= \frac{1}{17} - 2\left(\frac{1}{9}\right) + 1$
$= \frac{1}{17} - \frac{2}{9} + 1$
$= \frac{1}{17} - \frac{2}{9} + \frac{9}{9}$
$= \frac{1}{17} + \frac{9-2}{9}$
$= \frac{1}{17} + \frac{7}{9}$
$= \frac{9}{153} + \frac{119}{153}$
$= \frac{128}{153}$

## Step 3: Numerical approximation

$\frac{128}{153} â‰ˆ 0.8366013072$

## Final result

The exact value of the definite integral is $\frac{128}{153}$, and the numerical approximation rounded to 10 decimal places is 0.8366013072.

{"answer": "\\frac{128}{153}", "numerical_answer": "0.8366013072"}