<think>
Okay, let's tackle this integral step by step. The integral given is from 1.0 to infinity of (x² - 1.0²)^(2 - 1/2) times e^(-0.5² x²) multiplied by the Hermite polynomial H_{2*2+1}(0.5x) dx. First, I need to parse all the components here.

So, simplifying the exponents and indices: 2 - 1/2 is 1.5, which is 3/2. The Hermite polynomial has an index of 2*2+1, which is 5. The argument of the Hermite polynomial is 0.5x. The exponential term is e^(-0.25x²) because 0.5 squared is 0.25. The integrand becomes (x² - 1)^(3/2) e^(-0.25x²) H_5(0.5x).

Hmm, Hermite polynomials often come up in integrals involving Gaussian functions, especially in physics contexts like quantum mechanics. The integral here might relate to some orthogonality or known integral formula involving Hermite polynomials. Let me recall if there's a standard integral that matches this form.

The standard orthogonality relation for Hermite polynomials is ∫_{-∞}^∞ H_n(x) H_m(x) e^{-x²} dx = √π 2^n n! δ_{nm}. But our integral is from 1 to infinity, not the entire real line, and the weight function here is e^{-0.25x²}, not e^{-x²}. Also, there's a (x² -1)^{3/2} term, which complicates things.

Wait, the term (x² -1)^{3/2} can be written as (x² -1)^{3/2} = (x -1)^{3/2} (x +1)^{3/2}, but that's not immediately helpful. Alternatively, maybe a substitution could help here. Let's consider changing variables to make the integral look more standard.

Let me think about substitution. Let’s set t = 0.5x, so x = 2t, dx = 2dt. Then, when x = 1.0, t = 0.5, and as x approaches infinity, t approaches infinity. The integral becomes:

∫_{0.5}^∞ ( (2t)^2 -1 )^{3/2} e^{-0.25*(2t)^2} H_5(t) * 2 dt

Simplify the terms:

(4t² -1)^{3/2} e^{-t²} H_5(t) * 2 dt

Hmm, that's ∫_{0.5}^∞ 2 (4t² -1)^{3/2} e^{-t²} H_5(t) dt. Not sure if that helps. The presence of (4t² -1)^{3/2} complicates things. Maybe another substitution? Let's see if there's a way to express (4t² -1)^{3/2} in terms of some orthogonal polynomials or functions.

Alternatively, perhaps integrating by parts. Hermite polynomials have derivatives that relate to lower-order Hermite polynomials. The generating function for Hermite polynomials is e^{2xt - t²} = ∑_{n=0}^∞ H_n(x) t^n /n!.

But I'm not sure if that's helpful here. Alternatively, maybe expanding the Hermite polynomial into a series. H_5(t) is a polynomial of degree 5. Let's recall that H_5(t) = 32t^5 - 160t^3 + 120t. So, H_5(t) = 32t^5 -160t^3 +120t. If I substitute that into the integral, we can write the integral term by term.

So, the integral becomes 2 ∫_{0.5}^∞ (4t² -1)^{3/2} e^{-t²} (32t^5 -160t^3 +120t) dt. Breaking this into three separate integrals:

2*32 ∫ t^5 (4t² -1)^{3/2} e^{-t²} dt - 2*160 ∫ t^3 (4t² -1)^{3/2} e^{-t²} dt + 2*120 ∫ t (4t² -1)^{3/2} e^{-t²} dt.

But integrating each of these terms from 0.5 to infinity seems challenging. The presence of (4t² -1)^{3/2} suggests that maybe a trigonometric substitution or hypergeometric functions might be involved. Alternatively, perhaps a substitution u = 4t² -1. Let's try that.

Let u = 4t² -1. Then du/dt = 8t, so dt = du/(8t). When t = 0.5, u = 4*(0.25) -1 = 1 -1 = 0. When t approaches infinity, u approaches infinity. So the limits become from u=0 to u=∞. Let's express t in terms of u: t = sqrt((u +1)/4) = (sqrt(u +1))/2.

Substituting into the integral, for example, take the first term:

2*32 ∫_{0.5}^∞ t^5 (4t² -1)^{3/2} e^{-t²} dt = 64 ∫_{0}^∞ [ (sqrt(u+1)/2 )^5 ] u^{3/2} e^{- ( (sqrt(u+1)/2 )^2 ) } * (du/(8t)).

Wait, since t = sqrt(u+1)/2, then 1/t = 2 / sqrt(u+1). So dt = du/(8t) = du/(8*(sqrt(u+1)/2)) ) = du/(4 sqrt(u+1)).

So substituting all that into the integral:

64 * ∫_{0}^∞ [ ( (sqrt(u+1)/2 )^5 ) * u^{3/2} * e^{ - ( (u +1)/4 ) } * (1/(4 sqrt(u+1))) ) ] du

Simplify term by term:

First, (sqrt(u+1)/2)^5 = (u+1)^{5/2} / 32.

Multiply by u^{3/2}: (u+1)^{5/2} u^{3/2} / 32.

Multiply by e^{- (u+1)/4 }.

Multiply by 1/(4 sqrt(u+1)): 1/(4 (u+1)^{1/2}).

So combining all factors:

64 * [1/(32 * 4)] ∫_{0}^∞ (u+1)^{5/2} u^{3/2} (u+1)^{-1/2} e^{- (u+1)/4 } du

Simplify exponents: (u+1)^{5/2 -1/2} = (u+1)^2.

So the integrand becomes (u+1)^2 u^{3/2} e^{- (u+1)/4 }.

The constants: 64 / (32 *4) = 64 / 128? Wait, 32*4=128, so 64/128 = 0.5.

So the first term becomes 0.5 ∫_{0}^∞ (u+1)^2 u^{3/2} e^{- (u+1)/4 } du.

Hmm, this seems complicated. Let's expand (u+1)^2 = u² + 2u +1. Then the integral becomes:

0.5 ∫_{0}^∞ (u² + 2u +1) u^{3/2} e^{- (u+1)/4 } du

= 0.5 e^{-1/4} ∫_{0}^∞ (u^{7/2} + 2u^{5/2} + u^{3/2}) e^{-u/4} du

Because e^{-(u+1)/4} = e^{-1/4} e^{-u/4}.

Now, each of these integrals is a gamma function. The integral of u^{k} e^{-u/4} du from 0 to ∞ is 4^{k+1} Γ(k+1). Let's check:

For ∫ u^{n} e^{-a u} du from 0 to ∞, it's Γ(n+1)/a^{n+1}. Here, a = 1/4, so it's Γ(n+1) / (1/4)^{n+1} ) = 4^{n+1} Γ(n+1).

So for the terms:

1. u^{7/2}: n = 7/2, so 4^{7/2 +1} Γ(7/2 +1) = 4^{9/2} Γ(9/2)
2. 2u^{5/2}: n=5/2, 2*4^{5/2 +1} Γ(5/2 +1) = 2*4^{7/2} Γ(7/2)
3. u^{3/2}: n=3/2, 4^{3/2 +1} Γ(3/2 +1) = 4^{5/2} Γ(5/2)

So putting it all together:

0.5 e^{-1/4} [4^{9/2} Γ(9/2) + 2*4^{7/2} Γ(7/2) + 4^{5/2} Γ(5/2) ]

Compute each term:

First, 4^{9/2} = (2^2)^{9/2} = 2^9 = 512. Γ(9/2) = (7/2)(5/2)(3/2)(1/2)√π = (105/16)√π.

Second term: 2*4^{7/2} = 2*(2^7) = 2*128 = 256. Wait, 4^{7/2} = (2^2)^{7/2} = 2^7 = 128. So 2*128 = 256. Γ(7/2) = (5/2)(3/2)(1/2)√π = (15/8)√π.

Third term: 4^{5/2} = 2^5 = 32. Γ(5/2) = (3/2)(1/2)√π = (3/4)√π.

So substituting:

0.5 e^{-1/4} [512*(105/16)√π + 256*(15/8)√π + 32*(3/4)√π ]

Calculate each coefficient:

512*(105/16) = (512/16)*105 = 32*105 = 3360

256*(15/8) = (256/8)*15 = 32*15 = 480

32*(3/4) = 24

So total inside the brackets: (3360 + 480 +24)√π = 3864√π

Multiply by 0.5 e^{-1/4}: 0.5 * 3864√π e^{-1/4} = 1932√π e^{-1/4}

So the first term is 1932√π e^{-1/4}

But wait, this is just the first part of the three terms from the Hermite polynomial expansion. The original integral was split into three parts: the first term (with t^5), the second (with t^3), and the third (with t). So we need to compute all three integrals similarly.

Wait, no. Wait, the first term after substitution was the first part of the Hermite polynomial. But actually, when we expanded H_5(t) into 32t^5 -160t^3 +120t, the entire integral was split into three separate integrals. So the calculation I just did was for the first integral (the 32t^5 term). Then there are two more integrals for the -160t^3 and +120t terms. So I need to repeat this process for the other two terms.

But this seems very tedious. Let me check if there's a smarter way. Alternatively, maybe there's an orthogonality condition or a generating function approach that can be used here.

Alternatively, perhaps the integral is zero due to orthogonality. Let me think. The standard orthogonality is for H_n(x) e^{-x²} over (-infty, infty). Here, our weight function is e^{-0.25x²} (x² -1)^{3/2} from 1 to infinity. Not sure if that's related to any standard orthogonal polynomial weight function.

Alternatively, maybe the integral representation of Hermite polynomials. H_n(x) can be expressed as (-1)^n e^{x²} d^n/dx^n e^{-x²}. Not sure if that helps here.

Alternatively, perhaps using the fact that (x² -1)^{3/2} is related to Gegenbauer polynomials or associated Legendre functions, but I'm not sure.

Alternatively, maybe changing variables to y = x^2 -1, but that might not help.

Wait, let's think about the integral from 1 to infinity of (x² -1)^{3/2} e^{-0.25x²} H_5(0.5x) dx. Let's denote a = 0.5x, so x = 2a, dx = 2da. Then when x=1, a=0.5, and as x approaches infinity, a approaches infinity. The integral becomes:

∫_{0.5}^∞ (4a² -1)^{3/2} e^{-a²} H_5(a) * 2 da

Hmm, this is similar to the integral we had before. The integrand is 2a)^2 -1)^{3/2} e^{-a²} H_5(a) * 2 da. Wait, but H_5(a) is a polynomial of degree 5. Maybe expanding (4a² -1)^{3/2} as a series?

But (4a² -1)^{3/2} can be written as (sqrt(4a² -1))^3. However, expanding this in terms of a series might not be straightforward. Alternatively, perhaps using a binomial expansion for (4a² -1)^{3/2} as a sum over k of (3/2 choose k) (4a²)^k (-1)^{3/2 -k}, but fractional binomial coefficients might complicate things.

Alternatively, perhaps using hypergeometric functions. The term (4a² -1)^{3/2} can be expressed in terms of hypergeometric functions, but I'm not sure.

Alternatively, perhaps integrating term by term after expanding H_5(a). Since H_5(a) is 32a^5 -160a^3 +120a, as I had before. So the integral becomes:

2 ∫_{0.5}^∞ (4a² -1)^{3/2} e^{-a²} (32a^5 -160a^3 +120a) da

Which is 2*32 ∫ (4a² -1)^{3/2} a^5 e^{-a²} da - 2*160 ∫ (4a² -1)^{3/2} a^3 e^{-a²} da + 2*120 ∫ (4a² -1)^{3/2} a e^{-a²} da, all from a=0.5 to infinity.

But integrating these terms seems difficult. Maybe substitution. Let's consider for each integral, let u = a². Then du = 2a da. But not sure. Alternatively, substitution t = a - something.

Alternatively, consider that (4a² -1)^{3/2} can be written as (2a -1)^{3/2} (2a +1)^{3/2}, but that might not help.

Alternatively, perhaps using integration by parts. Let's take the first integral: ∫ (4a² -1)^{3/2} a^5 e^{-a²} da. Let’s set u = (4a² -1)^{3/2} a^4, dv = a e^{-a²} da. Then du would be complicated derivatives, but maybe manageable.

Alternatively, note that the integrand has a combination of polynomials and exponentials. Maybe look for a substitution that can convert it into a gamma function or beta function form.

Alternatively, consider that for a >= 0.5, 4a² -1 = (2a -1)(2a +1). Let’s set t = 2a -1. Then when a=0.5, t=0, and as a approaches infinity, t approaches infinity. Then 2a +1 = t + 2. So 4a² -1 = t(t + 2). Then a = (t +1)/2. da = dt/2.

Substituting into the first integral:

∫_{0}^∞ [t(t + 2)]^{3/2} * ((t +1)/2)^5 e^{- ((t +1)/2)^2 } * (dt/2)

This seems even more complicated. Maybe not helpful.

Alternatively, perhaps numerical integration is the way to go, but the problem asks for an analytical solution. So there must be a trick here.

Wait, let's recall that the integral involves H_{5}(0.5x) and the weight function (x² -1)^{3/2} e^{-0.25x²}. This might be related to some orthogonality in a different basis. Alternatively, perhaps using the integral representation of Hermite polynomials.

Another thought: The integral might be zero due to orthogonality. For example, if the function (x² -1)^{3/2} e^{-0.25x²} is an even function, and H_5}(0.5x) is an odd function, then the product might be even or odd. Let's check:

H_5(y) is an odd function since H_n(-y) = (-1)^n H_n(y). So H_5(-y) = -H_5(y). The argument here is 0.5x, and the integration is from x=1 to infinity. However, the function (x² -1)^{3/2} is even in x around x=0, but our integration is from x=1 to infinity, so x is positive. The exponential term e^{-0.25x²} is even. So the integrand is (x² -1)^{3/2} e^{-0.25x²} H_5(0.5x). H_5(0.5x) is a degree 5 polynomial, which is odd if x is replaced by -x. But since x is from 1 to infinity, which is all positive, the parity argument might not directly apply.

Alternatively, perhaps expanding H_5(0.5x) in terms of x and then integrating term by term. Let's try that.

H_5(y) = 32y^5 - 160y^3 + 120y. So H_5(0.5x) = 32*(0.5x)^5 -160*(0.5x)^3 +120*(0.5x) = 32*(x^5/32) -160*(x^3/8) +120*(x/2) = x^5 - 20x^3 + 60x. Wait, let's compute each term:

32*(0.5x)^5 = 32*(1/32)x^5 = x^5

-160*(0.5x)^3 = -160*(1/8)x^3 = -20x^3

120*(0.5x) = 60x

So H_5(0.5x) = x^5 -20x^3 +60x.

So the integrand becomes (x² -1)^{3/2} e^{-0.25x²} (x^5 -20x^3 +60x).

Therefore, the integral is ∫_{1}^∞ (x² -1)^{3/2} e^{-0.25x²} (x^5 -20x^3 +60x) dx.

Now, split this into three integrals:

I1 = ∫_{1}^∞ x^5 (x² -1)^{3/2} e^{-0.25x²} dx

I2 = -20 ∫_{1}^∞ x^3 (x² -1)^{3/2} e^{-0.25x²} dx

I3 = 60 ∫_{1}^∞ x (x² -1)^{3/2} e^{-0.25x²} dx

So the total integral is I1 + I2 + I3.

Now, perhaps each of these integrals can be expressed in terms of gamma functions or other special functions. Let's consider a substitution for each integral.

Let’s make a substitution t = x² -1. Then x² = t +1, x = sqrt(t +1), dx = (1/(2 sqrt(t +1))) dt. When x=1, t=0; as x approaches infinity, t approaches infinity.

So for I1:

I1 = ∫_{0}^∞ (t)^{3/2} e^{-0.25(t +1)} ( (sqrt(t +1))^5 ) * (1/(2 sqrt(t +1))) dt

Simplify the terms:

(t)^{3/2} e^{-0.25(t +1)} ( (t +1)^{5/2} ) * (1/(2 (t +1)^{1/2} )) dt

Combine exponents:

(t)^{3/2} (t +1)^{5/2 -1/2} = t^{3/2} (t +1)^{2}

So I1 = (1/2) e^{-0.25} ∫_{0}^∞ t^{3/2} (t +1)^2 e^{-0.25 t} dt

Similarly, expand (t +1)^2 = t² + 2t +1:

I1 = (1/2) e^{-0.25} ∫_{0}^∞ t^{3/2} (t² + 2t +1) e^{-0.25 t} dt

= (1/2) e^{-0.25} [ ∫ t^{7/2} e^{-0.25 t} dt + 2 ∫ t^{5/2} e^{-0.25 t} dt + ∫ t^{3/2} e^{-0.25 t} dt ]

Each of these integrals is a gamma function. Recall that ∫_{0}^∞ t^{k} e^{-a t} dt = Γ(k+1)/a^{k+1}

Here, a = 0.25, so:

For the first integral: k =7/2, Γ(9/2)/ (0.25)^{9/2 +1} = Γ(9/2)/ (0.25)^{11/2}

Wait, no: ∫ t^{k} e^{-a t} dt = Γ(k+1)/a^{k+1}

So for the first term, k=7/2:

Γ(7/2 +1)/ (0.25)^{7/2 +1} = Γ(9/2)/ (0.25)^{9/2}

Similarly for the others:

Second term: k=5/2, Γ(7/2)/ (0.25)^{7/2}

Third term: k=3/2, Γ(5/2)/ (0.25)^{5/2}

So compute each:

Γ(9/2) = (7/2)(5/2)(3/2)(1/2)√π = (105/16)√π

Γ(7/2) = (5/8)√π * 8? Wait, Γ(n+1) = n Γ(n). So Γ(1/2) = √π, Γ(3/2) = (1/2)√π, Γ(5/2) = (3/4)√π, Γ(7/2) = (15/8)√π, Γ(9/2) = (105/16)√π.

So:

First term: Γ(9/2)/ (0.25)^{9/2} = (105/16)√π / ( (1/4)^{9/2} )

(1/4)^{9/2} = (1/2^2)^{9/2} = 1/2^9 = 1/512

So 1/ (1/512) = 512. So (105/16)√π * 512 = (105 * 512/16)√π = 105 * 32√π = 3360√π

Second term: 2 * Γ(7/2)/ (0.25)^{7/2} = 2*(15/8)√π / (1/4)^{7/2}

(1/4)^{7/2} = 1/2^7 = 1/128. So 1/(1/128) = 128. So 2*(15/8)*128√π = 2*15*16√π = 480√π

Third term: Γ(5/2)/ (0.25)^{5/2} = (3/4)√π / (1/4)^{5/2}

(1/4)^{5/2} = 1/2^5 = 1/32. So 1/(1/32) =32. So (3/4)*32√π =24√π

So I1 = (1/2) e^{-0.25} (3360√π + 480√π +24√π) = (1/2) e^{-0.25} (3864√π) = 1932 e^{-0.25} √π

Similarly, compute I2:

I2 = -20 ∫_{1}^∞ x^3 (x² -1)^{3/2} e^{-0.25x²} dx

Again, substitution t = x² -1, x² = t +1, x = sqrt(t +1), dx = (1/(2 sqrt(t +1))) dt

So x^3 = (t +1)^{3/2}

Thus, I2 = -20 ∫_{0}^∞ t^{3/2} e^{-0.25(t +1)} (t +1)^{3/2} * (1/(2 sqrt(t +1))) dt

Simplify:

= -20*(1/2) e^{-0.25} ∫_{0}^∞ t^{3/2} (t +1)^{3/2 -1/2} e^{-0.25 t} dt

= -10 e^{-0.25} ∫_{0}^∞ t^{3/2} (t +1)^{1} e^{-0.25 t} dt

Expand (t +1) = t +1:

= -10 e^{-0.25} [ ∫_{0}^∞ t^{5/2} e^{-0.25 t} dt + ∫_{0}^∞ t^{3/2} e^{-0.25 t} dt ]

Compute each integral:

First integral: Γ(7/2)/ (0.25)^{7/2} = (15/8)√π / (1/4)^{7/2} = (15/8)√π * 128 = 240√π

Second integral: Γ(5/2)/ (0.25)^{5/2} = (3/4)√π *32 =24√π

So I2 = -10 e^{-0.25} (240√π +24√π) = -10 e^{-0.25} *264√π = -2640 e^{-0.25} √π

Now I3:

I3 =60 ∫_{1}^∞ x (x² -1)^{3/2} e^{-0.25x²} dx

Again, substitution t =x² -1, x= sqrt(t +1), dx= (1/(2 sqrt(t +1))) dt

x = sqrt(t +1), so x (x² -1)^{3/2} = sqrt(t +1) * t^{3/2}

Thus, I3 =60 ∫_{0}^∞ t^{3/2} sqrt(t +1) e^{-0.25(t +1)} * (1/(2 sqrt(t +1))) dt

Simplify:

=60*(1/2) e^{-0.25} ∫_{0}^∞ t^{3/2} e^{-0.25 t} dt

=30 e^{-0.25} ∫_{0}^∞ t^{3/2} e^{-0.25 t} dt

This integral is Γ(5/2)/ (0.25)^{5/2} = (3/4)√π *32 =24√π

So I3 =30 e^{-0.25} *24√π =720 e^{-0.25} √π

Now, summing I1 + I2 + I3:

1932 e^{-0.25} √π -2640 e^{-0.25} √π +720 e^{-0.25} √π

= (1932 -2640 +720) e^{-0.25} √π

Calculate the coefficients:

1932 -2640 = -708

-708 +720 =12

So total integral is 12 e^{-0.25} √π

Therefore, the exact answer is 12 e^{-1/4} √π.

Now, compute the numerical approximation:

First, compute e^{-1/4} ≈ e^{-0.25} ≈ 0.7788007830

√π ≈ 1.7724538509

Multiply all together: 12 * 0.7788007830 *1.7724538509

First, 0.7788007830 *1.7724538509 ≈ 1.380388447

Then, 12 *1.380388447 ≈16.564661364

Rounded to 10 decimal places: 16.564661364 ≈16.5646613640

But let me verify the calculation step by step to ensure no arithmetic errors.

First, e^{-0.25}:

e^{-0.25} ≈ 0.778800783071404868245

√π ≈1.772453850905516027298

Multiply these two: 0.778800783071404868245 *1.772453850905516027298

Let's compute this:

0.778800783071404868245 *1.772453850905516027298

Approximately:

0.7788 *1.77245 ≈

0.7788 *1 =0.7788

0.7788 *0.7 =0.54516

0.7788 *0.07 =0.054516

0.7788 *0.00245≈0.001908

Sum: 0.7788 +0.54516=1.32396 +0.054516=1.378476 +0.001908≈1.380384

So approximately 1.380384

Then multiply by 12: 1.380384 *12 =16.564608

Rounded to 10 decimal places: 16.5646080000, but let's compute more accurately.

Using exact values:

e^{-0.25} ≈0.778800783071404868245

√π ≈1.772453850905516027298

Multiply:

0.778800783071404868245 *1.772453850905516027298

Let's compute this using more precision:

First, 0.778800783071404868245 *1.772453850905516027298

Break it down:

=0.778800783071404868245 *1 =0.778800783071404868245

+0.778800783071404868245 *0.7 =0.5451605481499834077715

+0.778800783071404868245 *0.07 =0.05451605481499834077715

+0.778800783071404868245 *0.002453850905516027298

Compute the last term:

0.778800783071404868245 *0.002453850905516027298 ≈

0.778800783071404868245 *0.002 =0.00155760156614280973649

0.778800783071404868245 *0.000453850905516027298 ≈

Approx 0.7788 *0.00045385 ≈0.0003533

Total ≈0.00155760156614280973649 +0.0003533 ≈0.0019109

So total sum:

0.778800783071404868245

+0.5451605481499834077715 =1.3239613312213882750165

+0.05451605481499834077715 =1.3784773860363866157937

+0.0019109 ≈1.3803882860363866157937

So approximately 1.3803882860

Multiply by 12:

1.3803882860 *12 =16.564659432

Rounded to 10 decimal places:16.5646594320

But let's check with calculator:

Using a calculator:

e^{-0.25} ≈0.778800783071404868245

√π ≈1.772453850905516027298

Product:0.778800783071404868245 *1.772453850905516027298 ≈1.38038844754

Multiply 1.38038844754 by 12:

1.38038844754 *12 =16.56466137048

So approximately 16.5646613705

Rounded to 10 decimal places:16.5646613705

But the exact answer is 12 e^{-1/4} √π, which is 12 * e^{-0.25} * sqrt(pi).

So the numerical value is approximately 16.5646613705, which rounds to 16.5646613705.

But let me check with a calculator for more precision.

Alternatively, use Python:

import math

exact = 12 * math.exp(-0.25) * math.sqrt(math.pi)

print(exact)

Let me compute this:

math.exp(-0.25) ≈0.7788007830714049

math.sqrt(math.pi)≈1.7724538509055159

12 *0.7788007830714049 *1.7724538509055159

First, 0.7788007830714049 *1.7724538509055159 =1.3803884475408953

Then, 1.3803884475408953 *12 =16.564661370490744

So approximately 16.5646613705, which rounds to 16.5646613705 when rounded to 10 decimal places.

Therefore, the exact answer is 12 e^{-1/4} √π, and the numerical approximation is approximately 16.5646613705.

But wait, the original integral was from x=1.0 to infinity. Did we make any mistake in the substitution steps?

Wait, when we did t =x² -1 substitution, the limits were correct (from 0 to infinity). The steps seem correct, and the final result is 12 e^{-1/4} √π. Let me verify with another approach.

Alternatively, consider that the integral might be related to the integral of (x² -a²)^{ν} e^{-b x²} H_n(c x) dx. Perhaps there's a formula in tables of integrals.

In Gradshteyn and Ryzhik, for example, section 7.3 might have integrals involving Hermite polynomials. Let me check.

In G&R, 7.3** integrals of the form ∫_{a}^∞ (x² -a²)^{c} e^{-b x²} H_n(x) dx.

But I don't have the exact reference, but perhaps there's a formula.

Alternatively, consider that the integral we computed step by step gives 12 e^{-1/4} √π. Let's check if this makes sense.

Given that the integral of a product of a polynomial and a weight function over an interval can sometimes result in a simple expression, especially if the polynomial is orthogonal with respect to some weight. However, in this case, the weight function (x² -1)^{3/2} e^{-0.25x²} is not a standard weight for Hermite polynomials, but the result simplifies nicely to 12 e^{-1/4} √π, which seems plausible.

Therefore, the exact answer is 12 e^{-1/4} √π, and the numerical value is approximately 16.5646613705.
</think>

{"answer": "12 \\sqrt{\\pi} e^{-\\frac{1}{4}}", "numerical_answer": "16.5646613705"}