To solve the definite integral 

\[
\int_{1.0}^\infty x(x^2 - 1.0^2)^{2 - 3/2} e^{-0.5^2 x^2} H_{2*2}(0.5x) \, dx,
\]

let's break it down step by step.

### Step 1: Simplify the Integrand
First, simplify the terms in the integrand:

1. \((x^2 - 1.0^2)^{2 - 3/2} = (x^2 - 1)^{-1/2} = \frac{1}{\sqrt{x^2 - 1}}\).
2. \(H_{2*2}(0.5x) = H_4(0.5x)\), where \(H_4\) is the 4th-order Hermite polynomial.
3. The Hermite polynomial \(H_4(y)\) is given by:
   \[
   H_4(y) = 16y^4 - 48y^2 + 12.
   \]
   Substituting \(y = 0.5x\):
   \[
   H_4(0.5x) = 16(0.5x)^4 - 48(0.5x)^2 + 12 = x^4 - 12x^2 + 12.
   \]
4. The exponential term is \(e^{-0.25x^2}\).

So the integrand simplifies to:
\[
x \cdot \frac{1}{\sqrt{x^2 - 1}} \cdot e^{-0.25x^2} \cdot (x^4 - 12x^2 + 12).
\]

### Step 2: Rewrite the Integral
The integral becomes:
\[
\int_{1.0}^\infty \frac{x(x^4 - 12x^2 + 12)}{\sqrt{x^2 - 1}} e^{-0.25x^2} \, dx.
\]

### Step 3: Change of Variables
Let \(u = x^2 - 1\), so \(du = 2x \, dx\) and \(x \, dx = \frac{du}{2}\). When \(x = 1\), \(u = 0\), and as \(x \to \infty\), \(u \to \infty\). The integral becomes:
\[
\int_{0}^\infty \frac{(u + 1)^2 - 12(u + 1) + 12}{\sqrt{u}} e^{-0.25(u + 1)} \cdot \frac{du}{2}.
\]
Simplify the numerator:
\[
(u + 1)^2 - 12(u + 1) + 12 = u^2 + 2u + 1 - 12u - 12 + 12 = u^2 - 10u + 1.
\]
So the integral is:
\[
\frac{1}{2} \int_{0}^\infty \frac{u^2 - 10u + 1}{\sqrt{u}} e^{-0.25(u + 1)} \, du.
\]
Simplify \(\frac{u^2 - 10u + 1}{\sqrt{u}}\):
\[
\frac{u^2}{\sqrt{u}} - \frac{10u}{\sqrt{u}} + \frac{1}{\sqrt{u}} = u^{3/2} - 10u^{1/2} + u^{-1/2}.
\]
Thus, the integral becomes:
\[
\frac{1}{2} e^{-0.25} \int_{0}^\infty \left(u^{3/2} - 10u^{1/2} + u^{-1/2}\right) e^{-0.25u} \, du.
\]

### Step 4: Evaluate the Integral
Each term is a gamma integral. Recall that:
\[
\int_{0}^\infty u^{k} e^{-a u} \, du = \frac{\Gamma(k + 1)}{a^{k + 1}}.
\]
For our integral:
1. For \(u^{3/2}\): \(k = 3/2\), \(a = 0.25\):
   \[
   \int_{0}^\infty u^{3/2} e^{-0.25u} \, du = \frac{\Gamma(5/2)}{(0.25)^{5/2}}.
   \]
2. For \(u^{1/2}\): \(k = 1/2\), \(a = 0.25\):
   \[
   \int_{0}^\infty u^{1/2} e^{-0.25u} \, du = \frac{\Gamma(3/2)}{(0.25)^{3/2}}.
   \]
3. For \(u^{-1/2}\): \(k = -1/2\), \(a = 0.25\):
   \[
   \int_{0}^\infty u^{-1/2} e^{-0.25u} \, du = \frac{\Gamma(1/2)}{(0.25)^{1/2}}.
   \]
Using \(\Gamma(5/2) = \frac{3}{4}\sqrt{\pi}\), \(\Gamma(3/2) = \frac{1}{2}\sqrt{\pi}\), and \(\Gamma(1/2) = \sqrt{\pi}\), we get:
\[
\frac{1}{2} e^{-0.25} \left(\frac{\frac{3}{4}\sqrt{\pi}}{(0.25)^{5/2}} - 10 \cdot \frac{\frac{1}{2}\sqrt{\pi}}{(0.25)^{3/2}} + \frac{\sqrt{\pi}}{(0.25)^{1/2}}\right).
\]
Simplify the powers of 0.25:
\[
(0.25)^{5/2} = (1/4)^{5/2} = 1/32, \quad (0.25)^{3/2} = 1/8, \quad (0.25)^{1/2} = 1/2.
\]
Substitute these:
\[
\frac{1}{2} e^{-0.25} \left(\frac{\frac{3}{4}\sqrt{\pi}}{1/32} - 10 \cdot \frac{\frac{1}{2}\sqrt{\pi}}{1/8} + \frac{\sqrt{\pi}}{1/2}\right) = \frac{1}{2} e^{-0.25} \left(24\sqrt{\pi} - 40\sqrt{\pi} + 2\sqrt{\pi}\right).
\]
Combine terms:
\[
\frac{1}{2} e^{-0.25} (-14\sqrt{\pi}) = -7\sqrt{\pi} e^{-0.25}.
\]

### Step 5: Numerical Approximation
Compute \(-7\sqrt{\pi} e^{-0.25}\) numerically:
\[
\sqrt{\pi} \approx 1.7724538509, \quad e^{-0.25} \approx 0.7788007831.
\]
Multiply:
\[
-7 \cdot 1.7724538509 \cdot 0.7788007831 \approx -9.6614188766.
\]

### Final Answer
The exact answer is \(-7\sqrt{\pi} e^{-1/4}\), and the numerical approximation is \(-9.6614188766\).

```json
{"answer": "-7 \\sqrt{\\pi} e^{-1/4}", "numerical_answer": "-9.6614188766"}
```