Let's solve the integral:
\[
I = \int_0^3 x^{-1/4}(3-x)^{-1/4}\cosh\left(2\sqrt{x(3-x)}\right)dx
\]

**Step 1: Substitution**

Let us use the substitution:
\[
x = 3\sin^2\theta, \quad dx = 6\sin\theta\cos\theta\,d\theta = 3\sin(2\theta)\,d\theta
\]
When \(x = 0\), \(\theta = 0\); when \(x = 3\), \(\sin^2\theta = 1 \implies \theta = \frac{\pi}{2}\).

Now,
\[
x^{-1/4} = (3\sin^2\theta)^{-1/4} = 3^{-1/4}\sin^{-1/2}\theta
\]
\[
(3-x)^{-1/4} = (3-3\sin^2\theta)^{-1/4} = (3\cos^2\theta)^{-1/4} = 3^{-1/4}\cos^{-1/2}\theta
\]
\[
\sqrt{x(3-x)} = \sqrt{3\sin^2\theta \cdot 3\cos^2\theta} = 3\sin\theta\cos\theta = \frac{3}{2}\sin(2\theta)
\]
So,
\[
\cosh\left(2\sqrt{x(3-x)}\right) = \cosh\left(3\sin(2\theta)\right)
\]

Putting it all together:
\[
I = \int_0^{\pi/2} 3^{-1/4}\sin^{-1/2}\theta \cdot 3^{-1/4}\cos^{-1/2}\theta \cdot \cosh\left(3\sin(2\theta)\right) \cdot 3\sin(2\theta)\,d\theta
\]
\[
= 3^{1 - 1/2} \int_0^{\pi/2} \sin^{-1/2}\theta \cos^{-1/2}\theta \sin(2\theta) \cosh\left(3\sin(2\theta)\right) d\theta
\]
\[
= 3^{1/2} \int_0^{\pi/2} \sin^{-1/2}\theta \cos^{-1/2}\theta \sin(2\theta) \cosh\left(3\sin(2\theta)\right) d\theta
\]

But \(\sin(2\theta) = 2\sin\theta\cos\theta\), so:
\[
\sin^{-1/2}\theta \cos^{-1/2}\theta \sin(2\theta) = 2\sin^{1/2}\theta \cos^{1/2}\theta
\]

So,
\[
I = 3^{1/2} \int_0^{\pi/2} 2\sin^{1/2}\theta \cos^{1/2}\theta \cosh\left(3\sin(2\theta)\right) d\theta
\]
\[
= 2\sqrt{3} \int_0^{\pi/2} \sin^{1/2}\theta \cos^{1/2}\theta \cosh\left(3\sin(2\theta)\right) d\theta
\]

**Step 2: Further simplification**

Let us use the double angle formula:
\[
\sin^{1/2}\theta \cos^{1/2}\theta = \left(\sin\theta\cos\theta\right)^{1/2} = \left(\frac{1}{2}\sin(2\theta)\right)^{1/2} = 2^{-1/2}\sin^{1/2}(2\theta)
\]

So,
\[
I = 2\sqrt{3} \int_0^{\pi/2} 2^{-1/2} \sin^{1/2}(2\theta) \cosh\left(3\sin(2\theta)\right) d\theta
\]
\[
= \sqrt{6} \int_0^{\pi/2} \sin^{1/2}(2\theta) \cosh\left(3\sin(2\theta)\right) d\theta
\]

Now, let \(u = 2\theta\), so when \(\theta = 0\), \(u = 0\); when \(\theta = \pi/2\), \(u = \pi\); \(d\theta = du/2\):

\[
I = \sqrt{6} \int_{u=0}^{u=\pi} \sin^{1/2}u \cosh(3\sin u) \cdot \frac{du}{2}
\]
\[
= \frac{\sqrt{6}}{2} \int_0^{\pi} \sin^{1/2}u \cosh(3\sin u) du
\]

**Step 3: Series expansion for cosh**

Recall:
\[
\cosh(3\sin u) = \sum_{n=0}^\infty \frac{[3\sin u]^{2n}}{(2n)!}
\]
So,
\[
I = \frac{\sqrt{6}}{2} \int_0^{\pi} \sin^{1/2}u \sum_{n=0}^\infty \frac{3^{2n} \sin^{2n}u}{(2n)!} du
\]
\[
= \frac{\sqrt{6}}{2} \sum_{n=0}^\infty \frac{3^{2n}}{(2n)!} \int_0^{\pi} \sin^{2n + 1/2}u du
\]

The integral:
\[
\int_0^{\pi} \sin^{k}u du = \sqrt{\pi} \frac{\Gamma\left(\frac{k+1}{2}\right)}{\Gamma\left(\frac{k}{2}+1\right)}
\]
So for \(k = 2n + 1/2\):
\[
\int_0^{\pi} \sin^{2n + 1/2}u du = \sqrt{\pi} \frac{\Gamma\left(n + \frac{5}{4}\right)}{\Gamma\left(n + \frac{7}{4}\right)}
\]

**Step 4: Final exact answer**

So,
\[
I = \frac{\sqrt{6}}{2} \sum_{n=0}^\infty \frac{3^{2n}}{(2n)!} \sqrt{\pi} \frac{\Gamma\left(n + \frac{5}{4}\right)}{\Gamma\left(n + \frac{7}{4}\right)}
\]
\[
= \frac{\sqrt{6\pi}}{2} \sum_{n=0}^\infty \frac{9^n}{(2n)!} \frac{\Gamma\left(n + \frac{5}{4}\right)}{\Gamma\left(n + \frac{7}{4}\right)}
\]

**Step 5: Numerical approximation**

Let us compute the first few terms:

For \(n=0\):
\[
\frac{9^0}{0!} \frac{\Gamma(5/4)}{\Gamma(7/4)} = 1 \cdot \frac{\Gamma(5/4)}{\Gamma(7/4)}
\]
\[
\Gamma(5/4) \approx 0.9064024771
\]
\[
\Gamma(7/4) \approx 0.9190625260
\]
\[
\frac{\Gamma(5/4)}{\Gamma(7/4)} \approx 0.9852608092
\]

For \(n=1\):
\[
\frac{9^1}{2!} \frac{\Gamma(9/4)}{\Gamma(11/4)}
\]
\[
9/2 = 4.5
\]
\[
\Gamma(9/4) \approx 1.133003096
\]
\[
\Gamma(11/4) \approx 1.225416703
\]
\[
\frac{1.133003096}{1.225416703} \approx 0.924572857
\]
\[
4.5 \times 0.924572857 \approx 4.160577857
\]

For \(n=2\):
\[
\frac{9^2}{4!} \frac{\Gamma(13/4)}{\Gamma(15/4)}
\]
\[
81/24 = 3.375
\]
\[
\Gamma(13/4) \approx 1.504575489
\]
\[
\Gamma(15/4) \approx 1.726213965
\]
\[
\frac{1.504575489}{1.726213965} \approx 0.871947
\]
\[
3.375 \times 0.871947 \approx 2.942320
\]

For \(n=3\):
\[
\frac{9^3}{6!} \frac{\Gamma(17/4)}{\Gamma(19/4)}
\]
\[
729/720 = 1.0125
\]
\[
\Gamma(17/4) \approx 2.011464
\]
\[
\Gamma(19/4) \approx 2.393888
\]
\[
\frac{2.011464}{2.393888} \approx 0.840047
\]
\[
1.0125 \times 0.840047 \approx 0.850895
\]

For \(n=4\):
\[
\frac{9^4}{8!} \frac{\Gamma(21/4)}{\Gamma(23/4)}
\]
\[
6561/40320 \approx 0.1627
\]
\[
\Gamma(21/4) \approx 2.755731
\]
\[
\Gamma(23/4) \approx 3.393872
\]
\[
\frac{2.755731}{3.393872} \approx 0.812193
\]
\[
0.1627 \times 0.812193 \approx 0.132166
\]

Sum up the first five terms:
\[
S \approx 0.9852608092 + 4.160577857 + 2.942320 + 0.850895 + 0.132166 \approx 9.071220
\]

Now, multiply by \(\frac{\sqrt{6\pi}}{2}\):

\[
\sqrt{6\pi} \approx \sqrt{18.84955592} \approx 4.3431457505
\]
\[
\frac{\sqrt{6\pi}}{2} \approx 2.1715728752
\]
\[
I \approx 2.1715728752 \times 9.071220 \approx 19.69101913
\]

Adding a few more terms will not change the result much, as the terms decrease rapidly.

**Step 6: Final JSON output**

```json
{"answer": "\\frac{\\sqrt{6\\pi}}{2} \\sum_{n=0}^\\infty \\frac{9^n}{(2n)!} \\frac{\\Gamma\\left(n + \\frac{5}{4}\\right)}{\\Gamma\\left(n + \\frac{7}{4}\\right)}", "numerical_answer": "19.6910191300"}
```