<think>
Okay, let's tackle this integral step by step. The problem is to compute the definite integral from -1 to 0 of 5 times (x^6 + x) to the fourth power dx. Hmm, that looks a bit intimidating at first glance, but maybe I can break it down.

First, I need to expand the expression (x^6 + x)^4. Expanding a binomial like this usually involves using the binomial theorem, which states that (a + b)^n = sum from k=0 to n of (n choose k) a^(n-k) b^k. Let me try applying that here.

So, a is x^6 and b is x, and n is 4. Let's compute each term:

When k=0: (4 choose 0)*(x^6)^4*x^0 = 1*x^24*1 = x^24
k=1: 4*(x^6)^3*x^1 = 4*x^18*x = 4x^19
k=2: 6*(x^6)^2*x^2 = 6*x^12*x^2 = 6x^14
k=3: 4*(x^6)^1*x^3 = 4*x^6*x^3 = 4x^9
k=4: 1*(x^6)^0*x^4 = 1*1*x^4 = x^4

Adding all these terms together: x^24 + 4x^19 + 6x^14 + 4x^9 + x^4. Then, the integrand is 5 times this, so we have 5x^24 + 20x^19 + 30x^14 + 20x^9 + 5x^4.

Now, the integral becomes the integral from -1 to 0 of each term summed up. Let's integrate term by term.

Integral of 5x^24 dx is 5*(x^25)/25 = (5/25)x^25 = (1/5)x^25.

Integral of 20x^19 dx is 20*(x^20)/20 = x^20.

Integral of 30x^14 dx is 30*(x^15)/15 = 2x^15.

Integral of 20x^9 dx is 20*(x^10)/10 = 2x^10.

Integral of 5x^4 dx is 5*(x^5)/5 = x^5.

So putting it all together, the antiderivative F(x) is:

(1/5)x^25 + x^20 + 2x^15 + 2x^10 + x^5.

Now, we need to evaluate this from -1 to 0. Let's compute F(0) first. Plugging in 0, each term becomes 0, so F(0) = 0.

Now, F(-1) is:

(1/5)(-1)^25 + (-1)^20 + 2*(-1)^15 + 2*(-1)^10 + (-1)^5.

Let's compute each term:

(-1)^25 = -1, so (1/5)(-1) = -1/5.

(-1)^20 = 1 (since even exponent), so that term is 1.

2*(-1)^15: (-1)^15 is -1, so 2*(-1) = -2.

2*(-1)^10: (-1)^10 is 1, so 2*1 = 2.

(-1)^5 = -1.

Adding all these terms:

-1/5 + 1 - 2 + 2 -1.

Let's compute step by step:

Start with -1/5 +1 = 4/5.

4/5 -2 = 4/5 -10/5 = -6/5.

-6/5 +2 = -6/5 +10/5 = 4/5.

4/5 -1 = 4/5 -5/5 = -1/5.

So F(-1) = -1/5.

Therefore, the definite integral is F(0) - F(-1) = 0 - (-1/5) = 1/5.

Wait, that's interesting. So the exact answer is 1/5. Let me check if I made any mistakes here.

Wait, when we compute the definite integral from a to b, it's F(b) - F(a). So here, since the integral is from -1 to 0, it's F(0) - F(-1). Which is 0 - (-1/5) = 1/5. That seems correct.

But let me verify the expansion again. Let me check if expanding (x^6 + x)^4 gives the terms. Let me compute (x^6 + x)^4:

First, (a + b)^4 = a^4 + 4a^3b + 6a^2b^2 +4ab^3 +b^4.

So substituting a = x^6, b = x:

a^4 = x^24

4a^3b = 4x^18 *x =4x^19

6a^2b^2 =6x^12 *x^2=6x^14

4ab^3=4x^6 *x^3=4x^9

b^4 =x^4

So yes, that's correct. Then multiplied by 5 gives 5x^24 +20x^19 +30x^14 +20x^9 +5x^4. Then term by term integration:

Integral of 5x^24 is (5/25)x^25 = x^25/5.

Integral of 20x^19 is (20/20)x^20 =x^20.

Integral of 30x^14 is (30/15)x^15=2x^15.

Integral of 20x^9 is (20/10)x^10=2x^10.

Integral of 5x^4 is (5/5)x^5 =x^5.

So the antiderivative is correct. Then evaluating at 0 gives 0. At -1:

Each term:

x^25/5: (-1)^25 is -1, so -1/5.

x^20: (-1)^20=1.

2x^15: 2*(-1)^15=2*(-1)=-2.

2x^10: 2*(1)=2.

x^5: (-1)^5=-1.

Adding them: -1/5 +1 -2 +2 -1 = (-1/5) + (1 -2 +2 -1) = (-1/5) +0 = -1/5. So F(-1) is -1/5. Then F(0) - F(-1) = 0 - (-1/5) =1/5. So the exact answer is 1/5, which is 0.2.

Wait, that's a very clean result. Let me check if there's another way to see this, maybe substitution. Let me think. Let u = x^5 +1? Wait, but the integrand is (x^6 +x)^4. Let me factor x from x^6 +x: x(x^5 +1). So (x^6 +x)^4 = x^4*(x^5 +1)^4. Then the integrand becomes 5x^4*(x^5 +1)^4. Hmm, maybe substitution here. Let me try that.

Let u = x^5 +1. Then du/dx =5x^4. So 5x^4 dx = du. Then the integral becomes ∫ u^4 du. But the limits would change. When x = -1, u = (-1)^5 +1 = -1 +1 =0. When x=0, u=0^5 +1=1. So the integral from x=-1 to x=0 becomes ∫ from u=0 to u=1 of u^4 du. Which is [u^5 /5] from 0 to1 = (1/5 -0) =1/5. Oh! That's a much simpler way. So the exact answer is indeed 1/5. So the previous steps were correct, but this substitution method is more straightforward. So the exact answer is 1/5, which is 0.2 numerically. So the numerical approximation is 0.2, which when rounded to 10 decimal places is 0.2000000000.

So the final answer is 1/5, and the numerical is 0.2 exactly. Therefore, the JSON should be {"answer": "\frac{1}{5}", "numerical_answer": "0.2000000000"}.
</think>

{"answer": "\\frac{1}{5}", "numerical_answer": "0.2000000000"}