<think>
Okay, so I need to compute the definite integral from 0 to 1 of [log(1/x)]^7 dx. Hmm, let's start by simplifying the integrand. Wait, log(1/x) is the same as -log(x), right? Because log(1/x) = -log(x). So the integrand becomes (-log(x))^7. Since the exponent is 7, which is odd, that would be - (log(x))^7. So the integral is the integral from 0 to 1 of - (log(x))^7 dx. But wait, actually, the original function is [log(1/x)]^7, which is (-log(x))^7. Since 7 is odd, that's - (log(x))^7. So the integral becomes the integral from 0 to 1 of - (log(x))^7 dx. But maybe it's easier to just keep it as [log(1/x)]^7, which is the same as (-log(x))^7, but perhaps substitution can help here.

I remember that integrals involving [log(1/x)]^n can be transformed using substitution. Let me think. Let’s make a substitution to simplify the integral. Let’s set t = -log(x), which would mean when x approaches 0, t approaches infinity, and when x = 1, t = 0. Wait, but the limits of integration are from 0 to 1. So if x is 0, t approaches infinity, and x=1, t=0. So the limits would reverse. Let me check that. If x = 1, then t = -log(1) = 0. If x approaches 0 from the right, then -log(x) approaches infinity. So the substitution would change the integral to an integral from infinity to 0. But we can reverse the limits and multiply by -1. Let me write that out.

Let t = -log(x), so dt/dx = -1/x. Then, solving for dx, we get dx = -x dt. But since x = e^{-t}, because t = -log(x) implies x = e^{-t}. So dx = -e^{-t} dt. Therefore, when we substitute, the integral becomes:

Integral from x=0 to x=1 of t^7 dx (since [log(1/x)]^7 = t^7). But substituting, we have:

Integral from t=∞ to t=0 of t^7 * (-e^{-t} dt). Reversing the limits and removing the negative sign, this becomes the integral from t=0 to t=∞ of t^7 e^{-t} dt.

Ah! That's the definition of the Gamma function. The Gamma function Γ(n+1) is the integral from 0 to ∞ of t^n e^{-t} dt. So here, n is 7, so Γ(8). And Γ(n+1) = n! for integer n. So Γ(8) = 7! = 5040. Therefore, the integral is 5040.

Wait, but let me check again. The original substitution: t = -log(x), so x = e^{-t}, dx = -e^{-t} dt. Then, the integral becomes:

∫_{x=0}^{1} [log(1/x)]^7 dx = ∫_{t=∞}^{0} t^7 * (-e^{-t} dt) = ∫_{0}^{∞} t^7 e^{-t} dt = Γ(8) = 7! = 5040. So yes, the exact value is 5040.

But wait, let me confirm the substitution steps again. The original integral is from 0 to 1. When x approaches 0, t approaches infinity, and x=1 gives t=0. So when x goes from 0 to 1, t goes from infinity to 0. So substituting, the integral becomes ∫_{∞}^{0} t^7 * e^{-t} * (-dt) which is the same as ∫_{0}^{∞} t^7 e^{-t} dt. So that's correct. So the integral is indeed Γ(8) = 7! = 5040. So the exact answer is 5040.

Now, the numerical approximation. 5040 is an integer, so the numerical approximation is 5040.0000000000. But maybe I should check if there's a mistake here. Wait, let me verify with a different approach. Let's consider integrating [log(1/x)]^n from 0 to 1. The general formula for ∫₀¹ (ln(1/x))ⁿ dx is n! So for n=7, it's 7! = 5040. That seems right. Let me check for a smaller n. For example, n=1: ∫₀¹ ln(1/x) dx = ∫₀¹ -ln(x) dx. The integral of -ln(x) dx from 0 to1 is known to be 1. Which is 1! =1. Similarly, for n=2, ∫₀¹ (ln(1/x))² dx = 2! =2. So yes, the pattern holds. Therefore, for n=7, it's 7! =5040. So the exact answer is 5040, and numerically that's 5040.0000000000. So the problem is solved.
</think>

{"answer": "5040", "numerical_answer": "5040.0000000000"}