Given:
\[
I = \int_0^1 x^{-3/4}(1-x)^{-3/4} \cos\left(2\sqrt{x(1-x)}\right)\,dx
\]

### Step 1: Symmetry and Substitution

Let \( x = \sin^2\theta \), so \( dx = 2\sin\theta\cos\theta d\theta \), and as \( x \) goes from 0 to 1, \( \theta \) goes from 0 to \( \pi/2 \):

\[
x = \sin^2\theta,\quad 1-x = \cos^2\theta,\quad \sqrt{x(1-x)} = \sin\theta\cos\theta = \frac12 \sin 2\theta
\]
So,
\[
dx = 2\sin\theta\cos\theta d\theta = \sin 2\theta d\theta
\]
Also,
\[
x^{-3/4} = (\sin^2\theta)^{-3/4} = (\sin\theta)^{-3/2}
\]
\[
(1-x)^{-3/4} = (\cos^2\theta)^{-3/4} = (\cos\theta)^{-3/2}
\]
So the integrand becomes:
\[
x^{-3/4} (1-x)^{-3/4} dx = (\sin\theta)^{-3/2} (\cos\theta)^{-3/2} (\sin 2\theta d\theta)
\]

\[
\sin 2\theta = 2\sin\theta\cos\theta
\]
So the whole product is:
\[
(\sin\theta)^{-3/2} (\cos\theta)^{-3/2} \cdot 2 \sin\theta\cos\theta d\theta = 2 (\sin\theta)^{-1/2}(\cos\theta)^{-1/2} d\theta
\]

And the cosine part:
\[
\cos(2\sqrt{x(1-x)}) = \cos(\sin 2\theta)
\]

But that's not quite right. In fact,
\[
\sqrt{x(1-x)} = \sin\theta\cos\theta = \frac12 \sin 2\theta ,\quad
2\sqrt{x(1-x)} = \sin 2\theta
\]
Thus:
\[
\cos(2\sqrt{x(1-x)}) = \cos(\sin 2\theta)
\]

Wait, that's not correct; actually,
\[
2\sqrt{x(1-x)} = \sin 2\theta
\]
Thus,
\[
\cos(2\sqrt{x(1-x)}) = \cos(\sin 2\theta)
\]

But the problem had \( \cos(2\sqrt{x(1-x)}) = \cos(\sin 2\theta) \).

So, the integral becomes:
\[
I = 2 \int_0^{\pi/2} (\sin\theta)^{-1/2}(\cos\theta)^{-1/2} \cos(\sin 2\theta) d\theta
\]

Now,
\[
(\sin\theta)^{-1/2}(\cos\theta)^{-1/2} = [\sin\theta\cos\theta]^{-1/2}
\]
So,
\[
I = 2 \int_0^{\pi/2} [\sin\theta\cos\theta]^{-1/2} \cos(\sin 2\theta) d\theta
\]

### Step 2: Substitute \( \sin 2\theta = t \)

Let \( t = \sin 2\theta,\  dt = 2\cos 2\theta d\theta \).

Alternatively, let’s try to express the integral in terms of Beta and Bessel functions.

#### Connection to Beta/Bessel functions

Let’s consider a known generalization. For positive \( \alpha, \beta \), and \( a > 0 \):
\[
\int_0^1 x^{\alpha-1} (1-x)^{\beta-1} \cos\big( a \sqrt{x(1-x)} \big) dx
\]
This can be expressed in terms of the Bessel function \( J_{\nu} \):
\[
= \frac{\Gamma(\alpha)\Gamma(\beta)}{\Gamma(\alpha+\beta)} \ {}_1F_2\left(\frac{\alpha+\beta}{2}; \alpha, \beta; -\frac{a^2}{4}\right)
\]
For this particular form, a more useful result (see e.g., Gradshteyn & Ryzhik 3.944.1):

\[
\int_0^1 x^{\mu-1}(1-x)^{\nu-1} \cos\big( 2c \sqrt{x(1-x)} \big) dx = \frac{ \sqrt{\pi} \, \Gamma(\mu+\nu) }{2^{\mu+\nu-1} \Gamma(\mu+\frac12) \Gamma(\nu)} J_{\mu-1/2}(c) {}_2F_1(\cdots)
\]
But that's not precisely the form we need.

Alternatively, consider a table entry (Gradshteyn & Ryzhik 3.944.4):

\[
\int_0^1 x^{\lambda-1}(1-x)^{\mu-1} \cos\left( a x + b(1-x) \right) dx = \cdots
\]
but this doesn't match our argument.

Let’s consider the substitution \( x = \frac{1-\cos\phi}{2} \). Then 
\[
dx = \frac{1}{2} \sin\phi d\phi
\]
\( x = \frac{1-\cos\phi}{2} \rightarrow 1-x = \frac{1+\cos\phi}{2} \)

Also,
\[
x(1-x) = \frac{1-\cos\phi}{2} \cdot \frac{1+\cos\phi}{2} = \frac{1-\cos^2\phi}{4} = \frac{\sin^2\phi}{4}
\]
so
\[
\sqrt{x(1-x)} = \frac{1}{2}\sin\phi
\]
Thus,
\[
2\sqrt{x(1-x)} = \sin\phi
\]

Now,
\[
x^{-3/4} = \left(\frac{1-\cos\phi}{2}\right)^{-3/4}, \qquad
(1-x)^{-3/4} = \left(\frac{1+\cos\phi}{2}\right)^{-3/4}
\]

\[
x^{-3/4}(1-x)^{-3/4} = 2^{3/2} (1-\cos\phi)^{-3/4} (1+\cos\phi)^{-3/4}
\]

\[
dx = \frac{1}{2}\sin\phi d\phi
\]

As \( x \) goes from 0 to 1, \( \phi \) goes from 0 to \( \pi \).

So,
\[
I = 2^{3/2} \frac{1}{2} \int_0^\pi (1-\cos\phi)^{-3/4}(1+\cos\phi)^{-3/4} \sin\phi \cos(\sin\phi) d\phi
\]
\[
= 2^{1/2} \int_0^\pi (1-\cos\phi)^{-3/4}(1+\cos\phi)^{-3/4} \sin\phi \cos(\sin\phi) d\phi
\]

Now observe that
\[
(1-\cos\phi)(1+\cos\phi) = 1-\cos^2\phi = \sin^2\phi
\]
Thus,
\[
(1-\cos\phi)^{-3/4}(1+\cos\phi)^{-3/4} = (\sin^2\phi)^{-3/4} = (\sin\phi)^{-3/2}
\]
Therefore,

\[
I = 2^{1/2} \int_0^\pi (\sin\phi)^{-3/2} \sin\phi \cos(\sin\phi) d\phi = 2^{1/2} \int_0^\pi (\sin\phi)^{-1/2} \cos(\sin\phi) d\phi
\]

Thus,

\[
I = \sqrt{2} \int_0^\pi (\sin\phi)^{-1/2} \cos(\sin\phi) d\phi
\]

### Step 3: Recognize the Integral

Let us check if this is a standard integral.
Consider the Laplace transform formula (Gradshteyn & Ryzhik 3.944):

\[
\int_0^\pi (\sin\theta)^{\mu - 1} \cos(a \sin\theta) d\theta = \sqrt{\pi} \left( \frac{2}{a} \right)^{\frac{\mu-1}{2}} \Gamma\left(\frac{\mu}{2}\right) J_{\frac{\mu-1}{2}}(a)
\]

Setting \( a = 1 \), \( \mu - 1 = -1/2 \implies \mu = 1/2 \):

\[
\int_0^\pi (\sin\theta)^{-1/2} \cos(\sin\theta) d\theta = \sqrt{\pi} \left(2\right)^{-1/4} \Gamma\left(\frac14\right) J_{-1/4}(1)
\]

But be careful: In the table, the formula is:

\[
\int_0^\pi (\sin\theta)^{\mu - 1} \cos(a \sin\theta) \, d\theta = \sqrt{\pi} \Gamma\left(\frac{\mu}{2}\right) \left( \frac{2}{a} \right)^{\frac{\mu-1}{2}} J_{(\mu-1)/2}(a)
\]

So plugging in, for our case, \( \mu-1 = -1/2 \implies \mu = 1/2 \):

\[
I_0 = \int_0^\pi (\sin\phi)^{-1/2} \cos(a\sin\phi) d\phi = \sqrt{\pi} \Gamma\left( \frac14 \right) \left( \frac{2}{a} \right)^{-1/4} J_{-1/4}(a)
\]

Wait: According to Gradshteyn & Ryzhik Eq. 3.944(3), we have:

\[
\int_0^\pi (\sin\theta)^{\mu-1}\cos(a\sin\theta)d\theta = \sqrt{\pi} \Gamma\left(\frac{\mu}{2}\right) \left( \frac{2}{a} \right)^{(\mu-1)/2} J_{(\mu-1)/2}(a)
\]

So for our case \( a = 1 \) and \( \mu-1 = -1/2 \implies \mu = 1/2 \):

\[
\int_0^\pi (\sin\theta)^{-1/2} \cos(\sin\theta) d\theta = \sqrt{\pi} \Gamma\left(\frac14\right) \left( 2 \right)^{-1/4} J_{-1/4}(1)
\]

But note \( \Gamma(\frac{\mu}{2}) = \Gamma(\frac{1}{4}) \).

Therefore, our integral is:

\[
I = \sqrt{2} \int_0^\pi (\sin\phi)^{-1/2} \cos(\sin\phi) d\phi = \sqrt{2} \cdot \sqrt{\pi} \Gamma\left( \frac{1}{4} \right) 2^{-1/4} J_{-1/4}(1)
\]

\[
= \sqrt{\pi} \; 2^{1/2 - 1/4} \Gamma\left(\frac14\right) J_{-1/4}(1)
\]
\[
= \sqrt{\pi} \; 2^{1/4} \Gamma\left(\frac14\right) J_{-1/4}(1)
\]

### Step 4: Numerical Evaluation

Now,
- \( \sqrt{\pi} \approx 1.7724538509 \)
- \( 2^{1/4} \approx 1.1892071150 \)
- \( \Gamma(\frac14) \approx 3.6256099082 \)
- \( J_{-1/4}(1) \approx 0.9320295956 \)

So,

First, multiply \( \sqrt{\pi} \) and \( 2^{1/4} \):

\[
1.7724538509 \times 1.1892071150 = 2.1082544710
\]

Then times \( \Gamma(1/4) \):

\[
2.1082544710 \times 3.6256099082 = 7.6450276941
\]

Now times \( J_{-1/4}(1) \):

\[
7.6450276941 \times 0.9320295956 = 7.1260472978
\]

Thus, the numerical value is approximately

\[
\boxed{7.1260472978}
\]

### Step 5: Final Answer in JSON Format

```json
{"answer": "\\sqrt{\\pi}\\;2^{1/4}\\;\\Gamma\\left(\\tfrac{1}{4}\\right) J_{-1/4}(1)", "numerical_answer": "7.1260472978"}
```