
To solve the definite integral \( \int_{0}^{2} x^{-1/2}(2-x)^{1/2}\left[1 - 0.5x(2-x)\right]^{1/2} \, dx \), we proceed as follows:

### Step 1: Simplify the Integrand
First, simplify the expression inside the square root:
\[
1 - 0.5x(2-x) = 1 - x + 0.5x^2 = 0.5(x^2 - 2x + 2)
\]
Thus, the integrand becomes:
\[
x^{-1/2}(2-x)^{1/2} \cdot \sqrt{0.5(x^2 - 2x + 2)} = \frac{1}{\sqrt{2}} x^{-1/2}(2-x)^{1/2} \sqrt{x^2 - 2x + 2}
\]

### Step 2: Substitution
Let \( x = 2t \), so \( dx = 2dt \), and the limits change from \( x=0 \) to \( t=0 \) and \( x=2 \) to \( t=1 \). Substituting \( x = 2t \):
\[
x^{-1/2} = (2t)^{-1/2}, \quad (2-x)^{1/2} = \sqrt{2(1-t)}, \quad x^2 - 2x + 2 = 4t^2 - 4t + 2 = 2(2t^2 - 2t + 1)
\]
The integral transforms to:
\[
\int_{0}^{1} (2t)^{-1/2} \cdot \sqrt{2(1-t)} \cdot \sqrt{0.5 \cdot 2(2t^2 - 2t + 1)} \cdot 2 \, dt
\]
Simplifying constants and terms, this reduces to:
\[
2 \int_{0}^{1} t^{-1/2}(1-t)^{1/2} \sqrt{2t^2 - 2t + 1} \, dt
\]

### Step 3: Relate to Elliptic Integrals
Further simplification and substitution (e.g., trigonometric substitutions) show the integral relates to the complete elliptic integral of the second kind \( E(m) \), where \( m \) is the parameter. Specifically, the integral simplifies to \( 2E\left(\frac{1}{2}\right) \), where \( E\left(\frac{1}{2}\right) \) is the complete elliptic integral of the second kind with parameter \( m = \frac{1}{2} \).

### Step 4: Numerical Approximation
The numerical value of \( E\left(\frac{1}{2}\right) \) is approximately \( 1.3506438810 \). Thus, the integral evaluates to:
\[
2 \times 1.3506438810 \approx 2.7012877620
\]

### Final Answer
The exact answer is \( 2E\left(\frac{1}{2}\right) \), and the numerical approximation is \( 2.7012877621 \) (rounded to 10 decimal places).

{"answer": "2E\\left(\\frac{1}{2}\\right)", "numerical_answer": "2.7012877621"}