To solve the definite integral \(\int\limits_{0}^{2} x \arctan\left(\sqrt{x(2-x)}\right) \, dx\), we will follow these steps:

### Step 1: Simplify the Integrand
First, observe that the argument of the arctangent function is \(\sqrt{x(2-x)}\). Notice that \(x(2-x) = 2x - x^2 = 1 - (x-1)^2\), so:
\[
\sqrt{x(2-x)} = \sqrt{1 - (x-1)^2}.
\]
Let’s make the substitution \(u = x - 1\), which implies \(du = dx\) and \(x = u + 1\). The limits of integration change as follows:
- When \(x = 0\), \(u = -1\).
- When \(x = 2\), \(u = 1\).

The integral becomes:
\[
\int_{-1}^{1} (u + 1) \arctan\left(\sqrt{1 - u^2}\right) \, du.
\]

### Step 2: Exploit Symmetry
The integrand \((u + 1) \arctan\left(\sqrt{1 - u^2}\right)\) can be split into two parts:
\[
\int_{-1}^{1} u \arctan\left(\sqrt{1 - u^2}\right) \, du + \int_{-1}^{1} \arctan\left(\sqrt{1 - u^2}\right) \, du.
\]
The first integral is an odd function integrated over a symmetric interval, so it evaluates to zero:
\[
\int_{-1}^{1} u \arctan\left(\sqrt{1 - u^2}\right) \, du = 0.
\]
Thus, the integral simplifies to:
\[
\int_{-1}^{1} \arctan\left(\sqrt{1 - u^2}\right) \, du.
\]

### Step 3: Simplify the Arctangent Expression
Let \(\theta = \arctan\left(\sqrt{1 - u^2}\right)\). Then:
\[
\tan \theta = \sqrt{1 - u^2}, \quad \text{so} \quad \sin \theta = \sqrt{1 - u^2}, \quad \cos \theta = u.
\]
However, this seems inconsistent. Instead, let’s consider the substitution \(u = \sin \phi\), where \(\phi \in [-\pi/2, \pi/2]\). Then:
\[
\sqrt{1 - u^2} = \cos \phi, \quad du = \cos \phi \, d\phi.
\]
The integral becomes:
\[
\int_{-\pi/2}^{\pi/2} \arctan\left(\cos \phi\right) \cos \phi \, d\phi.
\]
Since \(\arctan\left(\cos \phi\right)\) is an even function, we can write:
\[
2 \int_{0}^{\pi/2} \arctan\left(\cos \phi\right) \cos \phi \, d\phi.
\]

### Step 4: Evaluate the Integral
To evaluate this integral, we use integration by parts. Let:
\[
v = \arctan\left(\cos \phi\right), \quad dv = -\frac{\sin \phi}{1 + \cos^2 \phi} \, d\phi,
\]
\[
dw = \cos \phi \, d\phi, \quad w = \sin \phi.
\]
Applying integration by parts:
\[
2 \left[ \sin \phi \arctan\left(\cos \phi\right) \Big|_{0}^{\pi/2} - \int_{0}^{\pi/2} \sin \phi \left(-\frac{\sin \phi}{1 + \cos^2 \phi}\right) \, d\phi \right].
\]
The boundary term evaluates to:
\[
\sin \phi \arctan\left(\cos \phi\right) \Big|_{0}^{\pi/2} = 1 \cdot \arctan(0) - 0 \cdot \arctan(1) = 0.
\]
Thus, the integral simplifies to:
\[
2 \int_{0}^{\pi/2} \frac{\sin^2 \phi}{1 + \cos^2 \phi} \, d\phi.
\]

### Step 5: Simplify the Integrand
Using the identity \(\sin^2 \phi = 1 - \cos^2 \phi\), the integrand becomes:
\[
\frac{1 - \cos^2 \phi}{1 + \cos^2 \phi} = \frac{2}{1 + \cos^2 \phi} - 1.
\]
Thus, the integral is:
\[
2 \left( 2 \int_{0}^{\pi/2} \frac{1}{1 + \cos^2 \phi} \, d\phi - \int_{0}^{\pi/2} 1 \, d\phi \right) = 4 \int_{0}^{\pi/2} \frac{1}{1 + \cos^2 \phi} \, d\phi - \pi.
\]

### Step 6: Evaluate the Remaining Integral
To evaluate \(\int_{0}^{\pi/2} \frac{1}{1 + \cos^2 \phi} \, d\phi\), we use the substitution \(t = \tan \phi\). Then:
\[
\cos^2 \phi = \frac{1}{1 + t^2}, \quad d\phi = \frac{dt}{1 + t^2}.
\]
The integral becomes:
\[
\int_{0}^{\infty} \frac{1}{1 + \frac{1}{1 + t^2}} \cdot \frac{dt}{1 + t^2} = \int_{0}^{\infty} \frac{1 + t^2}{2 + t^2} \cdot \frac{dt}{1 + t^2} = \int_{0}^{\infty} \frac{dt}{2 + t^2}.
\]
This evaluates to:
\[
\frac{1}{\sqrt{2}} \arctan\left(\frac{t}{\sqrt{2}}\right) \Big|_{0}^{\infty} = \frac{\pi}{2\sqrt{2}}.
\]
Thus, the original integral is:
\[
4 \cdot \frac{\pi}{2\sqrt{2}} - \pi = \frac{2\pi}{\sqrt{2}} - \pi = \pi \left( \sqrt{2} - 1 \right).
\]

### Step 7: Numerical Approximation
The exact answer is \(\pi \left( \sqrt{2} - 1 \right)\). Numerically:
\[
\sqrt{2} \approx 1.4142135624, \quad \pi \approx 3.1415926536,
\]
\[
\pi \left( \sqrt{2} - 1 \right) \approx 3.1415926536 \times 0.4142135624 \approx 1.3010767194.
\]

### Final Answer
```json
{"answer": "\\pi \\left( \\sqrt{2} - 1 \\right)", "numerical_answer": "1.3010767194"}
```