We start with the integral

  I = ∫₀⁷ [∛(√(x² + 1) + x) – ∛(√(x² + 1) – x)] dx.

Step 1. Define
  a = ∛(√(x² + 1) + x)  and  b = ∛(√(x² + 1) – x).

Notice that
  a³ = √(x² + 1) + x  and  b³ = √(x² + 1) – x.
Thus,
  a³ – b³ = (√(x² + 1) + x) – (√(x² + 1) – x) = 2x.

Also, the product is
  a · b = ∛[(√(x² + 1) + x)(√(x² + 1) – x)] = ∛(x² + 1 – x²) = ∛1 = 1.

Step 2. Let y = a – b. Then, using the identity for the cube of a difference,
  (a – b)³ = a³ – b³ – 3ab(a – b).
That is,
  y³ = 2x – 3·(1)·y  ⟹  y³ + 3y = 2x.
Rearrange to express x in terms of y:
  x = (y³ + 3y)/2.

Differentiate both sides with respect to y:
  dx/dy = (3y² + 3)/2 = (3(y² + 1))/2.
So, dx = [3(y² + 1)/2] dy.

Step 3. Change the integration limits in terms of y.
When x = 0:
  x = (y³ + 3y)/2 = 0  ⟹  y(y² + 3) = 0  ⟹  y = 0.
When x = 7:
  7 = (y³ + 3y)/2  ⟹  y³ + 3y = 14.
Testing y = 2:
  2³ + 3·2 = 8 + 6 = 14;  so y = 2.
Thus, the new limits are y = 0 to y = 2.

Step 4. Rewrite the original integral in terms of y:
Since the integrand is y and dx = [3(y² + 1)/2] dy, we have
  I = ∫₀² y · [3(y² + 1)/2] dy = (3/2) ∫₀² y (y² + 1) dy.
Expand the integrand:
  y (y² + 1) = y³ + y.
So,
  I = (3/2) [∫₀² y³ dy + ∫₀² y dy].

Now compute the integrals:
  ∫₀² y³ dy = [y⁴/4]₀² = (16/4) = 4,
  ∫₀² y dy = [y²/2]₀² = (4/2) = 2.
Thus, the sum is 4 + 2 = 6, and so
  I = (3/2) × 6 = 9.

Step 5. Final answers:
Exact answer: 9.
Numerical approximation (to 10 decimal places): 9.0000000000.

{"answer": "$9$", "numerical_answer": "9.0000000000"}