

To solve the definite integral \(\int_0^1 \frac{\ln\left(x + x^{-1}\right)}{x + x^{-1}} \, dx\), we proceed as follows:

### Step 1: Simplify the integrand
First, rewrite \(x + x^{-1}\) as \(\frac{x^2 + 1}{x}\). Thus, the logarithm term becomes:
\[
\ln\left(x + x^{-1}\right) = \ln\left(\frac{x^2 + 1}{x}\right) = \ln(x^2 + 1) - \ln x.
\]
The integrand then simplifies to:
\[
\frac{\ln(x^2 + 1) - \ln x}{\frac{x^2 + 1}{x}} = \frac{x\left(\ln(x^2 + 1) - \ln x\right)}{x^2 + 1} = \frac{x \ln(x^2 + 1)}{x^2 + 1} - \frac{x \ln x}{x^2 + 1}.
\]
The integral splits into two parts:
\[
\int_0^1 \frac{\ln\left(x + x^{-1}\right)}{x + x^{-1}} \, dx = \int_0^1 \frac{x \ln(x^2 + 1)}{x^2 + 1} \, dx - \int_0^1 \frac{x \ln x}{x^2 + 1} \, dx.
\]
Let these be \(I_1\) and \(I_2\), respectively.

### Step 2: Evaluate \(I_1\)
For \(I_1 = \int_0^1 \frac{x \ln(x^2 + 1)}{x^2 + 1} \, dx\), use the substitution \(u = x^2 + 1\), so \(du = 2x \, dx\) (i.e., \(x \, dx = \frac{du}{2}\)). When \(x = 0\), \(u = 1\); when \(x = 1\), \(u = 2\). Thus:
\[
I_1 = \frac{1}{2} \int_1^2 \frac{\ln u}{u} \, du.
\]
The integral \(\int \frac{\ln u}{u} \, du = \frac{1}{2} (\ln u)^2 + C\). Evaluating from \(1\) to \(2\):
\[
I_1 = \frac{1}{2} \left[ \frac{(\ln 2)^2}{2} - \frac{(\ln 1)^2}{2} \right] = \frac{(\ln 2)^2}{4} \cdot 2 = \frac{(\ln 2)^2}{2}.
\]

### Step 3: Evaluate \(I_2\)
For \(I_2 = \int_0^1 \frac{x \ln x}{x^2 + 1} \, dx\), use the substitution \(t = x^2\), so \(dt = 2x \, dx\) (i.e., \(x \, dx = \frac{dt}{2}\)). When \(x = 0\), \(t = 0\); when \(x = 1\), \(t = 1\). Also, \(\ln x = \frac{1}{2} \ln t\). Thus:
\[
I_2 = \int_0^1 \frac{x \ln x}{x^2 + 1} \, dx = \frac{1}{2} \int_0^1 \frac{\frac{1}{2} \ln t}{t + 1} \, dt = \frac{1}{4} \int_0^1 \frac{\ln t}{t + 1} \, dt.
\]
The integral \(\int_0^1 \frac{\ln t}{t + 1} \, dt\) is a known result. Using the power series expansion \(\frac{1}{t + 1} = \sum_{n=0}^\infty (-1)^n t^n\) (valid for \(|t| < 1\)) and integrating term-by-term, we find:
\[
\int_0^1 \frac{\ln t}{t + 1} \, dt = -\sum_{n=0}^\infty \frac{(-1)^n}{(n + 1)^2} = -\frac{\pi^2}{12}.
\]
Thus:
\[
I_2 = \frac{1}{4} \left(-\frac{\pi^2}{12}\right) = -\frac{\pi^2}{48}.
\]

### Step 4: Combine results
The original integral is \(I_1 - I_2\):
\[
\int_0^1 \frac{\ln\left(x + x^{-1}\right)}{x + x^{-1}} \, dx = \frac{(\ln 2)^2}{2} - \left(-\frac{\pi^2}{48}\right) = \frac{(\ln 2)^2}{2} + \frac{\pi^2}{48}.
\]

### Numerical Approximation
Using \(\ln 2 \approx 0.69314718056\) and \(\pi^2 \approx 9.8696044\):
\[
\frac{(\ln 2)^2}{2} \approx \frac{(0.69314718056)^2}{2} \approx 0.24022650695,
\]
\[
\frac{\pi^2}{48} \approx \frac{9.8696044}{48} \approx 0.2056167583.
\]
Adding these gives:
\[
0.24022650695 + 0.2056167583 \approx 0.44584326525.
\]

{"answer": "\\frac{\\pi^2}{48} + \\frac{(\\ln 2)^2}{2}", "numerical_answer": "0.4458432652"}