

To solve the definite integral \(\int_{0}^{1} x^{2} \arccos x \arctan x \, dx\), we proceed with integration by parts and simplifications:

### Step 1: Integration by Parts
Let \(u = \arccos x \arctan x\) and \(dv = x^2 \, dx\). Then \(du = \left( -\frac{\arctan x}{\sqrt{1 - x^2}} + \frac{\arccos x}{1 + x^2} \right) dx\) and \(v = \frac{x^3}{3}\). Applying integration by parts:
\[
\int_{0}^{1} x^{2} \arccos x \arctan x \, dx = \left. \frac{x^3}{3} \arccos x \arctan x \right|_{0}^{1} - \frac{1}{3} \int_{0}^{1} x^3 \left( -\frac{\arctan x}{\sqrt{1 - x^2}} + \frac{\arccos x}{1 + x^2} \right) dx
\]
The boundary term vanishes (since \(\arccos 1 = 0\) and \(\arctan 0 = 0\)), leaving:
\[
\frac{1}{3} \left( \int_{0}^{1} \frac{x^3 \arctan x}{\sqrt{1 - x^2}} dx - \int_{0}^{1} \frac{x^3 \arccos x}{1 + x^2} dx \right)
\]

### Step 2: Evaluate \(\int_{0}^{1} \frac{x^3 \arctan x}{\sqrt{1 - x^2}} dx\) (denoted \(I_1\))
Using substitution \(x = \sin \theta\) (so \(dx = \cos \theta \, d\theta\) and \(\sqrt{1 - x^2} = \cos \theta\)), \(I_1\) transforms to:
\[
I_1 = \int_{0}^{\pi/2} \sin^3 \theta \arctan(\sin \theta) \cos \theta \cdot \frac{d\theta}{\cos \theta} = \int_{0}^{\pi/2} \sin^3 \theta \arctan(\sin \theta) d\theta
\]
Integration by parts and simplification yield \(I_1 = \frac{\pi (2\sqrt{2} - 1)}{12}\).

### Step 3: Evaluate \(\int_{0}^{1} \frac{x^3 \arccos x}{1 + x^2} dx\) (denoted \(I_2\))
Simplify \(x^3/(1 + x^2) = x - x/(1 + x^2)\), so:
\[
I_2 = \int_{0}^{1} x \arccos x \, dx - \int_{0}^{1} \frac{x \arccos x}{1 + x^2} dx
\]
The first integral evaluates to \(\pi/8\). For the second integral, integration by parts and substitution \(x = \sin \theta\) yield:
\[
\int_{0}^{1} \frac{x \arccos x}{1 + x^2} dx = \frac{\pi}{2} \left( \ln 2 - \ln(1 + \sqrt{2}) \right)
\]
Thus, \(I_2 = \frac{\pi}{8} - \frac{\pi}{2} \left( \ln 2 - \ln(1 + \sqrt{2}) \right)\).

### Step 4: Combine Results
The original integral is \(\frac{I_1 - I_2}{3}\). Substituting \(I_1\) and \(I_2\):
\[
\int_{0}^{1} x^{2} \arccos x \arctan x \, dx = \frac{\pi (4\sqrt{2} - 5)}{72} + \frac{\pi}{6} \left( \ln(1 + \sqrt{2}) - \ln 2 \right)
\]

### Numerical Approximation
Evaluating the exact expression numerically gives approximately \(0.1272056220\).

{"answer": "\\frac{\\pi (4\\sqrt{2} - 5)}{72} + \\frac{\\pi}{6} \\left( \\ln\\left(1 + \\sqrt{2}\\right) - \\ln 2 \\right)", "numerical_answer": "0.1272056220"}