<think>
Okay, let's tackle this integral step by step. The integral given is from 0 to 2 of [x^(-1/2)(2 - x)^(-1/2) / sqrt(1 + x(2 - x)) times T_3(sqrt(1 + x(2 - x))) dx]. Hmm, that looks a bit complicated, but maybe there's a substitution that can simplify things.

First, let me parse the integrand. The numerator is x^(-1/2)(2 - x)^(-1/2), which reminds me of the Beta function or maybe a substitution involving trigonometric functions. The denominator is sqrt(1 + x(2 - x)). Let me compute the expression inside the square root first: 1 + x(2 - x) = 1 + 2x - x^2. Wait, that can be rewritten as -x^2 + 2x + 1. Let me check if that's a perfect square or something. Let's complete the square: -x^2 + 2x + 1 = -(x^2 - 2x) + 1 = -(x^2 - 2x +1 -1) +1 = -(x -1)^2 +2. So, 1 + x(2 - x) = 2 - (x -1)^2. So sqrt(2 - (x -1)^2). That looks like the equation of a circle with radius sqrt(2) centered at (1,0). Maybe a trigonometric substitution here?

But before that, let's also consider the T_3 term. T_3 is the third Chebyshev polynomial of the first kind. The Chebyshev polynomials T_n(x) are defined as T_n(cosθ) = cos(nθ). So, T_3(y) = 4y^3 - 3y. Let me confirm that: T_0(x) = 1, T_1(x) = x, T_2(x) = 2x^2 -1, T_3(x) = 4x^3 -3x. Yes, that's right. So, if we have T_3(sqrt(1 + x(2 -x))), that would be 4*(sqrt(1 + x(2 -x)))^3 - 3*sqrt(1 + x(2 -x)). So, substituting y = sqrt(1 + x(2 -x)), then T_3(y) = 4y^3 -3y. Maybe substituting y in terms of x could help.

But let's look at the entire integrand. Let me write it out:

Integral from 0 to 2 of [x^{-1/2} (2 - x)^{-1/2} / sqrt(1 + x(2 -x)) * T_3(sqrt(1 + x(2 -x)))] dx.

So, combining the terms, maybe we can make a substitution to simplify the expression. Let's consider substitution variables. Let me try to simplify the expression under the square root first. As we saw, 1 + x(2 -x) = 2 - (x -1)^2. Let me set t = x -1, so that substitution would make the expression sqrt(2 - t^2). But the limits of integration would change from x=0 to x=2, so t would go from -1 to 1. Then, x = t +1, dx = dt. Let's see if that helps.

But the other terms in the integrand are x^{-1/2}(2 -x)^{-1/2}. Let's substitute x = t +1. Then x = t +1, so 2 -x = 2 - (t +1) = 1 - t. So x^{-1/2}(2 -x)^{-1/2} = (t +1)^{-1/2}(1 - t)^{-1/2}. Hmm, that's [(1 - t^2)]^{-1/2} times (t +1)^{-1/2}(1 - t)^{-1/2}? Wait, (t +1)(1 - t) = 1 - t^2. So, (t +1)^{-1/2}(1 - t)^{-1/2} = (1 - t^2)^{-1/2}. So the x^{-1/2}(2 -x)^{-1/2} term becomes (1 - t^2)^{-1/2}. Then, the denominator is sqrt(2 - t^2). So the entire integrand becomes (1 - t^2)^{-1/2} / sqrt(2 - t^2) * T_3(sqrt(2 - t^2)) dt. Wait, but T_3(sqrt(2 - t^2)) is 4*(sqrt(2 - t^2))^3 - 3*sqrt(2 - t^2). So, substituting all that, the integrand becomes:

(1 - t^2)^{-1/2} / sqrt(2 - t^2) * [4*(2 - t^2)^{3/2} - 3*(2 - t^2)^{1/2}] dt.

Simplify each term:

First term: 4*(2 - t^2)^{3/2} / [sqrt(1 - t^2) * sqrt(2 - t^2)] = 4*(2 - t^2)^{(3/2 - 1/2)} / sqrt(1 - t^2) = 4*(2 - t^2)^1 / sqrt(1 - t^2) = 4*(2 - t^2)/sqrt(1 - t^2).

Second term: -3*(2 - t^2)^{1/2} / [sqrt(1 - t^2) * sqrt(2 - t^2)] = -3*(2 - t^2)^{0} / sqrt(1 - t^2) = -3 / sqrt(1 - t^2).

So combining both terms, the integrand becomes [4*(2 - t^2) - 3] / sqrt(1 - t^2) dt. Let's compute the numerator:

4*(2 - t^2) -3 = 8 -4t^2 -3 = 5 -4t^2.

Therefore, the integral becomes integral from t = -1 to t =1 of (5 -4t^2)/sqrt(1 - t^2) dt.

That's a much simpler integral! So now, the problem reduces to computing ∫_{-1}^{1} (5 -4t^2)/sqrt(1 - t^2) dt.

This is a standard integral. Let's split it into two parts: 5 ∫_{-1}^{1 1/sqrt(1 - t^2) dt -4 ∫_{-1}^{1} t^2 / sqrt(1 - t^2) dt.

First integral: 5 times the integral of 1/sqrt(1 - t^2) from -1 to1. The integral of 1/sqrt(1 - t^2) is arcsin(t), so evaluated from -1 to1, that's arcsin(1) - arcsin(-1) = π/2 - (-π/2) = π. So first term is 5π.

Second integral: -4 times the integral of t^2 / sqrt(1 - t^2) from -1 to1. Let's compute that integral. Let me note that the integrand is even function (t^2 is even, sqrt(1 - t^2) is even, so the whole integrand is even). So we can compute 2 times integral from 0 to1 of t^2 / sqrt(1 - t^2) dt. But since the original limits are from -1 to1, the integral is 2 times the integral from 0 to1. So, let's compute ∫ t^2 / sqrt(1 - t^2) dt. Let me use substitution. Let t = sinθ, so dt = cosθ dθ, sqrt(1 - t^2) = cosθ. Then the integral becomes ∫ sin²θ / cosθ * cosθ dθ = ∫ sin²θ dθ. Which is ∫ (1 - cos2θ)/2 dθ = (θ/2 - sin2θ/4) + C. Evaluated from θ=0 to θ=π/2. At θ=π/2, sinθ=1, so upper limit: (π/4 - 0) = π/4. Lower limit 0. So the integral from 0 to1 is π/4. Therefore, the integral from -1 to1 is 2*(π/4) = π/2. Therefore, the second term is -4*(π/2) = -2π.

Therefore, combining both terms: 5π -2π = 3π. So the integral is 3π.

Wait, so the entire original integral simplifies to 3π. Let me check the steps again to make sure.

Original substitution: x = t +1, so t goes from -1 to1. The integrand transformed correctly? Let's verify:

Original integrand: x^{-1/2}(2 -x)^{-1/2} / sqrt(1 +x(2 -x)) * T_3(sqrt(1 +x(2 -x))) dx.

After substitution x = t +1, dx = dt. Then x^{-1/2}(2 -x)^{-1/2} = (t +1)^{-1/2}(1 -t)^{-1/2} = (1 - t^2)^{-1/2}. The denominator sqrt(1 +x(2 -x)) = sqrt(2 - t^2). Then T_3(sqrt(2 - t^2)) = 4*(sqrt(2 - t^2))^3 -3*sqrt(2 - t^2). So multiplying all together:

(1 - t^2)^{-1/2} / sqrt(2 - t^2) * [4*(2 - t^2)^{3/2} -3*(2 - t^2)^{1/2}] dt.

Simplify each term:

First term: 4*(2 - t^2)^{3/2} / [sqrt(1 - t^2) * sqrt(2 - t^2)] = 4*(2 - t^2)^{(3/2 -1/2)} / sqrt(1 - t^2) = 4*(2 - t^2)^1 / sqrt(1 - t^2) = 4*(2 - t^2)/sqrt(1 - t^2).

Second term: -3*(2 - t^2)^{1/2} / [sqrt(1 - t^2) * sqrt(2 - t^2)] = -3*(2 - t^2)^{0}/sqrt(1 - t^2) = -3/sqrt(1 - t^2).

So combining, the integrand is [4*(2 - t^2) -3]/sqrt(1 - t^2) dt = [8 -4t^2 -3]/sqrt(1 - t^2) dt = (5 -4t^2)/sqrt(1 - t^2) dt. Correct.

Then integrating from -1 to1. Split into 5/sqrt(1 - t^2) -4t^2/sqrt(1 - t^2). The first integral is 5π, the second is -4*(π/2) = -2π. So total 3π. That seems right.

Therefore, the exact answer is 3π. The numerical approximation would be 3 * 3.1415926535... which is approximately 9.42477796077. Rounded to 10 decimal places, that's 9.4247779608.

Wait, let me check the numerical value. π is approximately 3.141592653589793. So 3π is 9.42477796076938. Rounded to 10 decimal places: 9.4247779608.

So the final answer is 3π, numerically approximately 9.4247779608.
</think>

{"answer": "3\\pi", "numerical_answer": "9.4247779608"}