To solve the definite integral \(\int_1^e x (\log x)^2 \, dx\), we will use integration by parts. Let's denote \(u = (\log x)^2\) and \(dv = x \, dx\).

### Step 1: Integration by Parts
First, we need to find \(du\) and \(v\):
- \(u = (\log x)^2\)
- \(dv = x \, dx\)

Differentiating \(u\) and integrating \(dv\):
- \(du = 2 \log x \cdot \frac{1}{x} \, dx = \frac{2 \log x}{x} \, dx\)
- \(v = \int x \, dx = \frac{x^2}{2}\)

Using the integration by parts formula \(\int u \, dv = uv - \int v \, du\):
\[
\int x (\log x)^2 \, dx = (\log x)^2 \cdot \frac{x^2}{2} - \int \frac{x^2}{2} \cdot \frac{2 \log x}{x} \, dx
\]

Simplify the integral:
\[
\int x (\log x)^2 \, dx = \frac{x^2 (\log x)^2}{2} - \int x \log x \, dx
\]

### Step 2: Solve the Remaining Integral
Now, we need to solve \(\int x \log x \, dx\) using integration by parts again. Let \(u = \log x\) and \(dv = x \, dx\):
- \(u = \log x\)
- \(dv = x \, dx\)

Differentiating \(u\) and integrating \(dv\):
- \(du = \frac{1}{x} \, dx\)
- \(v = \frac{x^2}{2}\)

Using the integration by parts formula again:
\[
\int x \log x \, dx = \log x \cdot \frac{x^2}{2} - \int \frac{x^2}{2} \cdot \frac{1}{x} \, dx
\]

Simplify the integral:
\[
\int x \log x \, dx = \frac{x^2 \log x}{2} - \int \frac{x}{2} \, dx = \frac{x^2 \log x}{2} - \frac{x^2}{4} + C
\]

### Step 3: Combine the Results
Substitute back into the original integral:
\[
\int x (\log x)^2 \, dx = \frac{x^2 (\log x)^2}{2} - \left( \frac{x^2 \log x}{2} - \frac{x^2}{4} \right) + C
\]

Simplify:
\[
\int x (\log x)^2 \, dx = \frac{x^2 (\log x)^2}{2} - \frac{x^2 \log x}{2} + \frac{x^2}{4} + C
\]

### Step 4: Evaluate the Definite Integral
Evaluate the integral from 1 to \(e\):
\[
\left[ \frac{x^2 (\log x)^2}{2} - \frac{x^2 \log x}{2} + \frac{x^2}{4} \right]_1^e
\]

At \(x = e\):
\[
\frac{e^2 (\log e)^2}{2} - \frac{e^2 \log e}{2} + \frac{e^2}{4} = \frac{e^2 \cdot 1^2}{2} - \frac{e^2 \cdot 1}{2} + \frac{e^2}{4} = \frac{e^2}{2} - \frac{e^2}{2} + \frac{e^2}{4} = \frac{e^2}{4}
\]

At \(x = 1\):
\[
\frac{1^2 (\log 1)^2}{2} - \frac{1^2 \log 1}{2} + \frac{1^2}{4} = \frac{1 \cdot 0^2}{2} - \frac{1 \cdot 0}{2} + \frac{1}{4} = 0 - 0 + \frac{1}{4} = \frac{1}{4}
\]

Subtract the two results:
\[
\frac{e^2}{4} - \frac{1}{4} = \frac{e^2 - 1}{4}
\]

### Step 5: Numerical Approximation
The numerical approximation of \(\frac{e^2 - 1}{4}\) is:
\[
\frac{e^2 - 1}{4} \approx \frac{7.38905609893065 - 1}{4} \approx \frac{6.38905609893065}{4} \approx 1.59726402473266
\]

### Final Answer
\[
\boxed{
\begin{aligned}
\text{"answer": "}\frac{e^2 - 1}{4}\text{"}, \\
\text{"numerical_answer": "1.5972640247"}
\end{aligned}
}
\]