Let's solve the integral:
\[
I = \int_{-4}^4 e^{|x|} \cdot \{x\} \, dx
\]
where \(\{x\} = x - \lfloor x \rfloor\) is the fractional part of \(x\).

---

### 1. Analyze the Integrand and the Interval

- The interval \([-4, 4]\) is symmetric around 0.
- The function \(e^{|x|}\) is even, while \(\{x\}\) is odd **about every integer**, but **not** about 0. The fractional part \(\{x\}\) is not an odd or even function.
- Note: For \(x < 0\), \(\{x\} = x - \lfloor x \rfloor\) is in \((0,1]\), since e.g. \(\{-1.2\} = -1.2 - (-2) = 0.8\).

---

### 2. Splitting the Interval

Let’s split the integral at 0:
\[
I = \int_{-4}^{0} e^{|x|} \{x\}\,dx + \int_0^4 e^{|x|} \{x\}\,dx
\]

Note that \(|x| = -x\) for \(x < 0\), \(|x| = x\) for \(x \geq 0\):

\[
I = \int_{-4}^{0} e^{-x} \{x\}\,dx + \int_0^4 e^{x} \{x\}\,dx
\]

---

#### For \(x \in [0,4]\):

\[
\{x\} = x - \lfloor x \rfloor
\]
Partition into the unit intervals:
\[
\int_0^4 e^{x} \{x\} dx = \sum_{k=0}^{3} \int_k^{k+1} e^{x} (x-k) dx
\]

---

#### For \(x \in [-4,0]\):

For \(x \in [-(k+1), -k]\), \(k=0,1,2,3\):
\[
x \in [-(k+1), -k] \implies \lfloor x \rfloor = -(k+1)
\]
So,
\[
\{x\} = x - (-(k+1)) = x + k + 1
\]
Therefore,

\[
\int_{-4}^0 e^{-x} \{x\} dx = \sum_{k=0}^{3} \int_{-(k+1)}^{-k} e^{-x} (x + k + 1) dx
\]

---

### 3. Write as a Sum

\[
I = \sum_{k=0}^3 \left[ \int_{-(k+1)}^{-k} e^{-x}(x + k + 1) dx + \int_{k}^{k+1} e^{x}(x - k) dx \right]
\]

---

#### Simplify Each Term

##### For \(k\) fixed:

- \(A_k = \int_{-(k+1)}^{-k} e^{-x}(x + k + 1) dx\)
- \(B_k = \int_{k}^{k+1} e^{x}(x - k) dx\)

Let's compute \(A_k\) and \(B_k\):

---

#### Compute \(B_k\):

Let \(u = x - k\), so \(x = k + u\), as \(x\) goes from \(k\) to \(k+1\), \(u\) goes from \(0\) to \(1\).

\[
B_k = \int_{k}^{k+1} e^{x}(x - k) dx = \int_0^1 e^{k + u} u du = e^k \int_0^1 e^{u} u du
\]

Compute \(\int_0^1 e^u u du\) via integration by parts:

Let
- \(u = u\), \(dv = e^u du\)
- \(du = du\), \(v = e^u\)

So:
\[
\int e^u u du = u e^u - \int e^u du = u e^u - e^u + C
\]

Apply endpoints:

\[
\int_0^1 e^u u du = (u e^u - e^u) \Big|_{u=0}^{u=1} = \left(1 \cdot e^1 - e^1\right) - \left(0 - e^0\right) = (e - e) - (-1) = 0 + 1 = 1
\]

So:
\[
B_k = e^k \cdot 1 = e^k
\]

---

#### Compute \(A_k\):

Let’s let \(x = -y\), where \(y\) runs from \(k+1\) down to \(k\) as \(x\) goes from \(-(k+1)\) to \(-k\).

So, \(dx = -dy\), \(x + k + 1 = -y + k + 1 = -(y - (k+1))\):

Let’s express \(x = -y\), so \(e^{-x} = e^{y}\):

So,
\[
A_k = \int_{-(k+1)}^{-k} e^{-x}(x + k + 1) dx = \int_{y=k+1}^{k} e^{y} \left[ - (y - (k+1)) \right] (-dy)
\]
\[
= \int_{y=k}^{k+1} e^{y} (y - (k+1)) dy
\]

So we now have,
\[
A_k = \int_{k}^{k+1} e^{y} (y - (k+1)) dy
\]

---

Therefore, for each \(k\), \(k=0,1,2,3\):

\[
I = \sum_{k=0}^3 \left[ \int_{k}^{k+1} e^{y} (y - (k+1)) dy + \int_{k}^{k+1} e^{y}(y - k) dy \right]
\]

Combine these two:

- \((y - (k+1)) + (y - k) = 2y - (2k + 1)\)

So,

\[
I = \sum_{k=0}^3 \int_{k}^{k+1} e^{y} \left[2y - (2k + 1) \right] dy
\]

Swap \(y\) to \(x\) for simplicity,

\[
I = \sum_{k=0}^3 \int_{x=k}^{k+1} e^{x} (2x - (2k + 1)) dx
\]

---

### 4. Integrate Each Term

For each \(k\):

\[
\int e^{x} (2x - (2k + 1)) dx
\]
Let’s do the indefinite integral:
\[
\int e^{x} 2x dx - \int e^{x} (2k + 1) dx = 2 \int x e^{x} dx - (2k + 1) \int e^{x} dx
\]

We know:
\[
\int x e^{x} dx = (x - 1) e^{x} + C
\]
So,
\[
2 \int x e^{x} dx = 2(x - 1) e^{x}
\]
and,
\[
\int e^{x} dx = e^{x}
\]

Therefore,
\[
\int e^{x} (2x - (2k + 1)) dx = 2(x - 1) e^{x} - (2k + 1) e^{x} + C = (2x - 2 - 2k - 1)e^{x} + C = (2x - 2k - 3)e^{x} + C
\]

Thus, over \([k, k+1]\), the definite integral is:
\[
\left[ (2x - 2k - 3) e^{x} \right]_{x=k}^{x=k+1}
\]
\[
= \left[ (2(k+1) - 2k -3) e^{k+1} - (2k - 2k -3) e^{k} \right]
\]
\[
= \left[ (2 -3) e^{k+1} - (-3) e^{k} \right]
= \left[ (-1) e^{k+1} + 3 e^{k} \right]
= 3 e^{k} - e^{k+1}
\]

---

### 5. Sum Over \(k=0,1,2,3\)

\[
I = \sum_{k=0}^3 \left(3e^{k} - e^{k+1} \right)
= 3\sum_{k=0}^3 e^{k} - \sum_{k=0}^3 e^{k+1}
\]

Compute each sum:

\[
\sum_{k=0}^3 e^{k} = e^{0} + e^{1} + e^{2} + e^{3}
\]
\[
\sum_{k=0}^3 e^{k+1} = e^{1} + e^{2} + e^{3} + e^{4}
\]

So,
\[
I = 3(e^{0} + e^{1} + e^{2} + e^{3}) - (e^{1} + e^{2} + e^{3} + e^{4})
\]

\[
= 3e^{0} + 3e^{1} + 3e^{2} + 3e^{3} - e^{1} - e^{2} - e^{3} - e^{4}
\]

\[
= 3e^{0} + (3e^{1} - e^{1}) + (3e^{2} - e^{2}) + (3e^{3} - e^{3}) - e^{4}
\]
\[
= 3e^{0} + 2e^{1} + 2e^{2} + 2e^{3} - e^{4}
\]
As \(e^{0} = 1\):

\[
\boxed{I = 3 + 2e + 2e^{2} + 2e^{3} - e^{4}}
\]

---

### 6. Numerical Approximation

Calculate each term (rounded to 10 decimal digits):

- \(e \approx 2.7182818285\)
- \(e^2 \approx 7.3890560989\)
- \(e^3 \approx 20.0855369232\)
- \(e^4 \approx 54.5981500331\)

So,
\[
I = 3 + 2 \times 2.7182818285 + 2 \times 7.3890560989 + 2 \times 20.0855369232 - 54.5981500331
\]
Step by step:

- \(2 \times 2.7182818285 = 5.4365636570\)
- \(2 \times 7.3890560989 = 14.7781121978\)
- \(2 \times 20.0855369232 = 40.1710738464\)

Now sum:

\[
I = 3 + 5.4365636570 + 14.7781121978 + 40.1710738464 - 54.5981500331
\]
\[
= (3 + 5.4365636570) = 8.4365636570
\]
\[
8.4365636570 + 14.7781121978 = 23.2146758548
\]
\[
23.2146758548 + 40.1710738464 = 63.3857497012
\]
\[
63.3857497012 - 54.5981500331 = 8.7875996681
\]

So, to 10 decimal digits:
\[
I \approx 8.7875996681
\]

---

### 7. Final JSON Answer

```json
{"answer": "3 + 2e + 2e^2 + 2e^3 - e^4", "numerical_answer": "8.7875996681"}
```