<think>
Okay, let's tackle this integral step by step. The integral given is:

∫₀¹ x^{0.5 - 1} (1 - x)^{2 - 2×0.5} (1 + x)^{-2} ln[(1 - x)/(1 + x)] ln[x/(1 - x)²] dx

First, I need to simplify the exponents. Let's compute them:

0.5 - 1 = -0.5, so the first term is x^{-0.5}.

For the second term, 2 - 2×0.5 = 2 - 1 = 1, so (1 - x)^1.

So the integral becomes:

∫₀¹ x^{-1/2} (1 - x) (1 + x)^{-2} ln[(1 - x)/(1 + x)] ln[x/(1 - x)²] dx

Hmm, that's a bit complicated. Let's see if we can manipulate the integrand or use substitution. The presence of logarithms suggests that differentiation under the integral sign might be useful here. Alternatively, maybe expanding the logarithms into simpler terms.

Looking at the logarithms:

ln[(1 - x)/(1 + x)] = ln(1 - x) - ln(1 + x)

ln[x/(1 - x)²] = ln x - 2 ln(1 - x)

So multiplying these two gives:

[ln(1 - x) - ln(1 + x)] [ln x - 2 ln(1 - x)]

Expanding this product:

ln(1 - x) * ln x - 2 [ln(1 - x)]² - ln(1 + x) * ln x + 2 ln(1 + x) ln(1 - x)

So the integral becomes the sum of four integrals:

I1 = ∫ x^{-1/2} (1 - x)(1 + x)^{-2} ln(1 - x) ln x dx

I2 = -2 ∫ x^{-1/2} (1 - x)(1 + x)^{-2} [ln(1 - x)]² dx

I3 = -∫ x^{-1/2} (1 - x)(1 + x)^{-2} ln(1 + x) ln x dx

I4 = 2 ∫ x^{-1/2} (1 - x)(1 + x)^{-2} ln(1 + x) ln(1 - x) dx

This seems quite involved. Maybe there's a smarter substitution or a known integral formula that can be applied here. Alternatively, perhaps using Beta functions or Gamma functions with differentiation with respect to parameters.

Let me recall that integrals of the form ∫₀¹ x^{c-1} (1 - x)^{d - c -1} (1 + x)^{-a} ... might relate to hypergeometric functions, but with the logarithms, it's more complicated. The logarithms can be thought of as derivatives of x^k or similar terms with respect to some parameter.

Alternatively, consider substitution. Let me try to make a substitution to simplify the terms. Let’s set t = x/(1 - x)^2. Wait, but that's inside one of the logarithms. Alternatively, maybe set t = (1 - x)/(1 + x), which is the argument of the first logarithm. Let's try that.

Let t = (1 - x)/(1 + x). Then solving for x:

t(1 + x) = 1 - x → t + t x = 1 - x → x(t + 1) = 1 - t → x = (1 - t)/(1 + t)

Then dx/dt: Let's compute derivative of x with respect to t.

dx/dt = [ - (1 + t) - (1 - t) ] / (1 + t)^2 = [ -1 - t -1 + t ] / (1 + t)^2 = (-2)/(1 + t)^2

So dx = -2/(1 + t)^2 dt

When x = 0, t = (1 - 0)/(1 + 0) = 1. When x = 1, t = (1 - 1)/(1 + 1) = 0. So the limits invert, and the integral becomes from t=1 to t=0, but with the negative sign, we can reverse the limits and drop the negative:

Integral becomes ∫₀¹ [ ( (1 - t)/(1 + t) )^{-1/2} (1 - (1 - t)/(1 + t)) (1 + (1 - t)/(1 + t))^{-2} ] * [ln t] * [ln ( ( (1 - t)/(1 + t) ) / (1 - (1 - t)/(1 + t))² ) ] * (2/(1 + t)^2) dt

This seems messy, but let's simplify each term step by step.

First, x = (1 - t)/(1 + t)

Compute x^{-1/2}:

x^{-1/2} = [ (1 - t)/(1 + t) ]^{-1/2} = [ (1 + t)/(1 - t) ]^{1/2}

Next, (1 - x) = 1 - (1 - t)/(1 + t) = [ (1 + t) - (1 - t) ] / (1 + t) = (2t)/(1 + t)

Then, (1 + x) = 1 + (1 - t)/(1 + t) = [ (1 + t) + (1 - t) ] / (1 + t) = 2/(1 + t)

So (1 + x)^{-2} = [2/(1 + t)]^{-2} = (1 + t)^2 / 4

Putting all these into the integrand:

[ (1 + t)/(1 - t) ]^{1/2} * (2t)/(1 + t) * (1 + t)^2 / 4 * [ln t] * [ln (x / (1 - x)^2 ) ] * 2/(1 + t)^2 dt

Wait, let me check each term:

Original integrand after substitution:

x^{-1/2} (1 - x) (1 + x)^{-2} * ln t * ln [x/(1 - x)^2] * 2/(1 + t)^2

So substituting each part:

x^{-1/2} = [ (1 + t)/(1 - t) ]^{1/2}

(1 - x) = 2t/(1 + t)

(1 + x)^{-2} = (2/(1 + t))^{-2} = (1 + t)^2 / 4? Wait, (2/(1 + t))^{-2} is ( (1 + t)/2 )^2 = (1 + t)^2 / 4? Wait, no. Wait, 2/(1 + t) raised to -2 is [ (1 + t)/2 ]^2? Wait, no. Wait, (a)^{-2} = 1/a². So (2/(1 + t))^{-2} = (1 + t)^2 / 4. Yes.

So (1 + x)^{-2} = (1 + t)^2 / 4.

Then, putting all together:

[ (1 + t)/(1 - t) ]^{1/2} * (2t/(1 + t)) * ( (1 + t)^2 / 4 ) * ln t * ln [x/(1 - x)^2 ] * 2/(1 + t)^2 dt

Now, let's simplify the coefficients:

First, multiply all the constants and the t terms:

(1 + t)^{1/2} / (1 - t)^{1/2} * 2t/(1 + t) * (1 + t)^2 / 4 * 2/(1 + t)^2

Wait, let's compute the exponents of (1 + t) and (1 - t):

Starting with (1 + t)/(1 - t) raised to 1/2: (1 + t)^{1/2} (1 - t)^{-1/2}

Multiply by (2t/(1 + t)): 2t (1 + t)^{-1}

Multiply by (1 + t)^2 / 4: (1 + t)^2 / 4

Multiply by 2/(1 + t)^2: 2/(1 + t)^2

So combining all the (1 + t) terms:

1/2 exponent from the first term, then -1 from the second term, +2 from the third term, -2 from the fourth term. So total exponent: 0.5 -1 +2 -2 = -0.5

Similarly, (1 - t) terms: -0.5 exponent from the first term, no others. So (1 - t)^{-0.5}

The constants: 2 from the second term, 1/4 from the third term, and 2 from the fourth term. So 2 * (1/4) * 2 = 1.

So overall, the non-logarithmic part simplifies to:

(1 + t)^{-0.5} (1 - t)^{-0.5} * t

Which is t / sqrt{(1 + t)(1 - t)} } = t / sqrt(1 - t²)

So the integrand becomes:

[ t / sqrt(1 - t²) ] * ln t * ln [x/(1 - x)^2 ] * dt

But we need to express ln [x/(1 - x)^2 ] in terms of t.

Recall x = (1 - t)/(1 + t), and 1 - x = 2t/(1 + t). So (1 - x)^2 = 4t²/(1 + t)^2

Thus, x/(1 - x)^2 = [ (1 - t)/(1 + t) ] / [4t²/(1 + t)^2 ] = [ (1 - t)(1 + t) ] / [4t² ] = (1 - t²)/(4t²)

Therefore, ln [x/(1 - x)^2 ] = ln( (1 - t²)/(4t²) ) = ln(1 - t²) - ln(4t²) = ln(1 - t²) - ln4 - 2 ln t

So substituting back into the integrand:

[ t / sqrt(1 - t²) ] * ln t * [ ln(1 - t²) - ln4 - 2 ln t ] dt

Therefore, the integral becomes:

∫₀¹ [ t / sqrt(1 - t²) ] * ln t * [ ln(1 - t²) - ln4 - 2 ln t ] dt

This seems more manageable. Let's split this into three integrals:

J1 = ∫₀¹ [ t / sqrt(1 - t²) ] * ln t * ln(1 - t²) dt

J2 = - ln4 ∫₀¹ [ t / sqrt(1 - t²) ] * ln t dt

J3 = -2 ∫₀¹ [ t / sqrt(1 - t²) ] * (ln t)^2 dt

So the original integral is J1 + J2 + J3.

Let's compute each of these integrals.

Starting with J2 and J3, as they might be simpler.

First, J2:

J2 = - ln4 ∫₀¹ [ t / sqrt(1 - t²) ] * ln t dt

Let’s make substitution u = 1 - t², then du = -2t dt, so t dt = -du/2

When t=0, u=1; t=1, u=0. So:

J2 = - ln4 ∫₁⁰ [ t / sqrt(u) ] * ln t * (-du/2t )

Simplify:

The t cancels, and the negative sign from du and the integral swap limits:

J2 = - ln4 * (1/2) ∫₀¹ [1 / sqrt(u)] ln t du

But we need to express ln t in terms of u. Since u = 1 - t², t = sqrt(1 - u). So ln t = (1/2) ln(1 - u)

Therefore:

J2 = - (ln4)/2 ∫₀¹ u^{-1/2} * (1/2) ln(1 - u) du

= - (ln4)/4 ∫₀¹ u^{-1/2} ln(1 - u) du

The integral ∫₀¹ u^{c -1} ln(1 - u) du is known. In general, ∫₀¹ x^{c-1} (1 - x)^{d -1} dx = B(c, d) = Γ(c)Γ(d)/Γ(c + d). If we differentiate with respect to d, we can get integrals involving ln(1 - x). Specifically,

d/dd B(c, d) = ∫₀¹ x^{c -1} (1 - x)^{d -1} ln(1 - x) dx = B(c, d) [ψ(d) - ψ(c + d)]

Where ψ is the digamma function.

In our case, the integral is ∫₀¹ u^{-1/2} ln(1 - u) du. Here, c = 1/2, d = 1 (since (1 - u)^{1 -1} = 1). So:

∫₀¹ u^{-1/2} ln(1 - u) du = B(1/2, 1) [ψ(1) - ψ(1/2 + 1)]

Compute B(1/2, 1) = Γ(1/2)Γ(1)/Γ(3/2) = sqrt(π) * 1 / ( (1/2) sqrt(π) ) ) = sqrt(π) / ( (sqrt(π)/2) ) = 2

Then ψ(1) = -γ (Euler-Mascheroni constant, approximately -0.5772, but exact value here), and ψ(3/2) = ψ(1/2) = ψ(1/2) + 2/(1) + 1/(1/2) ? Wait, no. The digamma function has the property ψ(z + 1) = ψ(z) + 1/z. So ψ(3/2) = ψ(1/2) + 2. We know ψ(1/2) = -γ - 2 ln 2. Therefore:

ψ(3/2) = -γ - 2 ln 2 + 2

Thus, ψ(1) - ψ(3/2) = (-γ) - [ -γ - 2 ln 2 + 2 ] = -γ + γ + 2 ln 2 - 2 = 2 ln 2 - 2

Therefore, the integral becomes:

B(1/2,1) [ψ(1) - ψ(3/2)] = 2 * (2 ln 2 - 2) = 4 ln 2 - 4

Therefore, J2 = - (ln4)/4 * (4 ln 2 - 4) = - (ln4) (ln 2 - 1)

But ln4 = 2 ln2, so:

J2 = -2 ln2 (ln2 - 1) = -2 (ln2)^2 + 2 ln2

Now, moving to J3:

J3 = -2 ∫₀¹ [ t / sqrt(1 - t²) ] (ln t)^2 dt

Again, let's use substitution u = 1 - t², du = -2t dt, t dt = -du/2

Then, when t=0, u=1; t=1, u=0. So:

J3 = -2 ∫₁⁰ [ t / sqrt(u) ] (ln t)^2 (-du/2t )

Simplify:

The t cancels, the negative from du and the integral limits swap:

J3 = -2 * (1/2) ∫₀¹ u^{-1/2} (ln t)^2 du

Again, t = sqrt(1 - u), so ln t = (1/2) ln(1 - u)

Thus, (ln t)^2 = (1/4) [ln(1 - u)]^2

Therefore:

J3 = - ∫₀¹ u^{-1/2} * (1/4) [ln(1 - u)]^2 du

= - (1/4) ∫₀¹ u^{-1/2} [ln(1 - u)]^2 du

This integral is more complicated. Let's recall that integrals of the form ∫₀¹ x^{c-1} (1 - x)^{d -1} [ln(1 - x)]^n dx can be expressed using higher derivatives of the Beta function. Specifically, taking multiple derivatives with respect to d.

But here, we have u^{-1/2} [ln(1 - u)]^2, which corresponds to c = 1/2, d =1, and n=2.

The general formula for the nth derivative of B(c, d) with respect to d is:

d^n/dd^n B(c, d) = ∫₀¹ x^{c -1} (1 - x)^{d -1} [ln(1 - x)]^n dx

So in our case, n=2, c=1/2, d=1:

∫₀¹ u^{-1/2} [ln(1 - u)]^2 du = d²/dd² B(1/2, d) evaluated at d=1

First, compute B(1/2, d) = Γ(1/2)Γ(d)/Γ(1/2 + d)

Then, the first derivative with respect to d:

d/dd B(1/2, d) = B(1/2, d) [ψ(d) - ψ(1/2 + d)]

Second derivative:

d²/dd² B(1/2, d) = B(1/2, d) [ (ψ'(d) - ψ'(1/2 + d)) + (ψ(d) - ψ(1/2 + d))^2 ]

Wait, actually, differentiating the first derivative:

d/dd [ B(1/2, d) (ψ(d) - ψ(1/2 + d)) ] = B(1/2, d) [ψ'(d) - ψ'(1/2 + d)] + B(1/2, d) (ψ(d) - ψ(1/2 + d)) * [ψ(d) - ψ(1/2 + d) - ψ(1/2 + d) - ψ(d) ] ?

Wait, no. Wait, the derivative of B(1/2, d) is B(1/2, d) [ψ(d) - ψ(1/2 + d)]. So the second derivative would be:

d/dd [ B(1/2, d) (ψ(d) - ψ(1/2 + d)) ] = B(1/2, d) [ψ'(d) - ψ'(1/2 + d)] + B(1/2, d) (ψ(d) - ψ(1/2 + d)) * [ψ(d) - ψ(1/2 + d) - ... ] ?

Wait, perhaps it's better to use the product rule:

Let’s denote B = B(1/2, d), and F = ψ(d) - ψ(1/2 + d)

Then d/dd (B F) = (d/dd B) F + B (d/dd F)

But d/dd B = B [ψ(d) - ψ(1/2 + d)] = B F

So d/dd (B F) = B F^2 + B (ψ’(d) - ψ’(1/2 + d))

Therefore, the second derivative is:

B F^2 + B (ψ’(d) - ψ’(1/2 + d))

Evaluated at d=1.

But when d=1, B(1/2,1) = 2 as before.

F at d=1 is ψ(1) - ψ(3/2) = (-γ) - (-γ - 2 ln2 + 2) = 2 ln2 - 2, as computed earlier.

ψ’(d) is the trigamma function. We know that ψ’(1) = π²/6, and ψ’(3/2) = π²/2 - 4.

Wait, let me recall specific values:

Trigamma function ψ’(z) has known values. For example:

ψ’(1) = π²/6 ≈ 1.6449...

ψ’(1/2) = π²/2 ≈ 4.9348...

ψ’(3/2) = ψ’(1/2) - 4 = π²/2 - 4 ≈ 0.9348...

Wait, actually, the recurrence relation for trigamma is ψ’(z + 1) = ψ’(z) - 1/z².

So ψ’(3/2) = ψ’(1/2) - 1/(1/2)^2 = ψ’(1/2) - 4 = π²/2 - 4 ≈ 4.9348 - 4 = 0.9348.

Therefore, ψ’(1) = π²/6, ψ’(3/2) = π²/2 - 4.

Thus, ψ’(1) - ψ’(3/2) = π²/6 - (π²/2 - 4) = -π²/3 + 4

Therefore, the second derivative at d=1 is:

B(1/2,1) [F^2 + (ψ’(1) - ψ’(3/2))] = 2 [ (2 ln2 - 2)^2 + (-π²/3 + 4) ]

So the integral ∫₀¹ u^{-1/2} [ln(1 - u)]^2 du = 2 [ (2 ln2 - 2)^2 + (-π²/3 + 4) ]

Therefore, J3 = -1/4 * 2 [ (2 ln2 - 2)^2 + (-π²/3 + 4) ] = -1/2 [ (2 ln2 - 2)^2 - π²/3 + 4 ]

Let's expand (2 ln2 - 2)^2:

= 4 (ln2)^2 - 8 ln2 + 4

So:

J3 = -1/2 [4 (ln2)^2 - 8 ln2 + 4 - π²/3 + 4 ]

= -1/2 [4 (ln2)^2 - 8 ln2 + 8 - π²/3 ]

= -2 (ln2)^2 + 4 ln2 - 4 + π²/6

Now, moving to J1:

J1 = ∫₀¹ [ t / sqrt(1 - t²) ] * ln t * ln(1 - t²) dt

This seems more complex. Let's try substitution here as well. Let’s set u = t², then du = 2t dt, so t dt = du/2. But not sure. Alternatively, set u = 1 - t², then du = -2t dt. Let's try that.

Let u = 1 - t², then du = -2t dt, t dt = -du/2. When t=0, u=1; t=1, u=0.

So J1 becomes:

∫₁⁰ [ t / sqrt(u) ] * ln t * ln(u) * (-du/2t )

Simplify:

The t cancels, and swap limits:

J1 = (1/2) ∫₀¹ u^{-1/2} ln t * ln u du

But t = sqrt(1 - u), so ln t = (1/2) ln(1 - u)

Thus:

J1 = (1/2) ∫₀¹ u^{-1/2} * (1/2) ln(1 - u) * ln u du

= (1/4) ∫₀¹ u^{-1/2} ln u ln(1 - u) du

This integral is non-trivial. Let's consider expanding ln(1 - u) as a series. Recall that ln(1 - u) = - Σ_{n=1}^∞ u^n / n for |u| < 1.

So:

J1 = - (1/4) ∫₀¹ u^{-1/2} ln u Σ_{n=1}^∞ u^n / n du

= - (1/4) Σ_{n=1}^∞ (1/n) ∫₀¹ u^{n - 1/2} ln u du

The integral ∫₀¹ u^{k} ln u du = -1/(k + 1)^2. Here, k = n - 1/2.

Thus:

J1 = - (1/4) Σ_{n=1}^∞ (1/n) [ -1/(n + 1/2)^2 ] = (1/4) Σ_{n=1}^∞ 1 / [n (n + 1/2)^2 ]

This series needs to be evaluated. Let's write it as:

Σ_{n=1}^∞ 1 / [n (n + 1/2)^2 ] = Σ_{n=1}^∞ 1 / [n (n + 1/2)^2 ]

Let’s consider partial fractions or relate it to known series. Let’s denote m = n + 1/2, then n = m - 1/2, but this might not help directly. Alternatively, write 1/[n(n + 1/2)^2] as partial fractions.

Let’s set:

1/[n(n + 1/2)^2] = A/n + B/(n + 1/2) + C/(n + 1/2)^2

Multiply both sides by n(n + 1/2)^2:

1 = A(n + 1/2)^2 + B n (n + 1/2) + C n

Expand:

A(n² + n + 1/4) + B(n² + n/2) + C n = 1

Group terms:

(A + B) n² + (A + B/2 + C) n + (A/4) = 1

Equate coefficients:

A + B = 0

A + B/2 + C = 0

A/4 = 1

From the last equation: A = 4

Then from first equation: 4 + B = 0 → B = -4

From second equation: 4 + (-4)/2 + C = 0 → 4 - 2 + C = 0 → C = -2

Thus:

1/[n(n + 1/2)^2] = 4/n - 4/(n + 1/2) - 2/(n + 1/2)^2

Therefore, the sum becomes:

Σ_{n=1}^∞ [4/n - 4/(n + 1/2) - 2/(n + 1/2)^2 ]

= 4 Σ_{n=1}^∞ 1/n - 4 Σ_{n=1}^∞ 1/(n + 1/2) - 2 Σ_{n=1}^∞ 1/(n + 1/2)^2

Let’s compute each series:

First series: Σ_{n=1}^∞ 1/n is the harmonic series, which diverges. Wait, but this can't be, since the original integral converges. There must be a mistake here. Wait, but we have partial fractions leading to divergent series? That can't be. Wait, perhaps the partial fraction decomposition is incorrect?

Wait, let's check the partial fractions again.

We have:

1 = A(n + 1/2)^2 + Bn(n + 1/2) + Cn

Expanding:

A(n² + n + 1/4) + B(n² + n/2) + Cn

= A n² + A n + A/4 + B n² + (B/2) n + C n

Grouping:

(A + B) n² + (A + B/2 + C) n + A/4 = 1

So:

A + B = 0

A = -B

A + B/2 + C = 0 → (-B) + B/2 + C = 0 → -B/2 + C = 0 → C = B/2

A/4 = 1 → A = 4

Thus, A=4, B=-4, C=-2. So the partial fractions are correct.

But then the sum becomes:

4 Σ 1/n -4 Σ 1/(n + 1/2) -2 Σ 1/(n + 1/2)^2

But Σ 1/n from n=1 to ∞ is divergent, but in our case, the original integral J1 is finite, so there must be cancellation of divergences. However, this suggests that the approach via expanding ln(1 - u) into a series might not be the best way here. Perhaps there's another method.

Alternatively, consider differentiating a Beta function with respect to two parameters. Let's recall that:

∫₀¹ x^{c -1} (1 - x)^{d -1} ln x ln(1 - x) dx = ∂²/(∂c ∂d) B(c, d)

But in our case, the integral is ∫₀¹ u^{-1/2} ln u ln(1 - u) du, which is similar to c = 1/2, d =1, but with the integrand x^{c -1} (1 - x)^{d -1} ln x ln(1 - x). So yes, this is the mixed partial derivative of B(c, d) with respect to c and d.

So:

∫₀¹ x^{c -1} (1 - x)^{d -1} ln x ln(1 - x) dx = ∂² B(c, d)/(∂c ∂d)

Therefore, for our case, c = 1/2, d =1:

J1 = (1/4) * ∂² B(1/2, 1)/(∂c ∂d) evaluated at c=1/2, d=1.

But B(c, d) = Γ(c)Γ(d)/Γ(c + d)

So, first, compute the partial derivatives.

First, compute ∂/∂c B(c, d) = B(c, d) [ψ(c) - ψ(c + d)]

Then, ∂²/(∂c ∂d) B(c, d) = ∂/∂d [ B(c, d) (ψ(c) - ψ(c + d)) ] = B(c, d) [ψ(c) - ψ(c + d)] [ψ(d) - ψ(c + d)] + B(c, d) [ - ψ’(c + d) ]

Therefore, at c=1/2, d=1:

∂² B/(∂c ∂d) = B(1/2,1) [ψ(1/2) - ψ(3/2)] [ψ(1) - ψ(3/2)] + B(1/2,1) [ - ψ’(3/2) ]

We already know:

B(1/2,1) = 2

ψ(1/2) = -γ - 2 ln2

ψ(3/2) = ψ(1/2) + 2 = -γ - 2 ln2 + 2

ψ(1) = -γ

ψ(1/2) - ψ(3/2) = (-γ - 2 ln2) - (-γ - 2 ln2 + 2) = -2

ψ(1) - ψ(3/2) = (-γ) - (-γ - 2 ln2 + 2) = 2 ln2 - 2

ψ’(3/2) = π²/2 - 4

Therefore:

∂² B/(∂c ∂d) = 2*(-2)*(2 ln2 - 2) + 2*(- (π²/2 - 4)) = 2*(-2)(2 ln2 - 2) - 2*(π²/2 - 4)

Compute each term:

First term: 2*(-2)(2 ln2 - 2) = -4 (2 ln2 - 2) = -8 ln2 + 8

Second term: -2*(π²/2 - 4) = -π² + 8

So total:

-8 ln2 + 8 - π² + 8 = -8 ln2 + 16 - π²

Therefore, the integral ∫₀¹ u^{-1/2} ln u ln(1 - u) du = ∂² B/(∂c ∂d) = -8 ln2 + 16 - π²

Thus, J1 = (1/4) * (-8 ln2 + 16 - π²) = -2 ln2 + 4 - π²/4

Now, combining all parts:

J1 + J2 + J3 = [ -2 ln2 + 4 - π²/4 ] + [ -2 (ln2)^2 + 2 ln2 ] + [ -2 (ln2)^2 + 4 ln2 - 4 + π²/6 ]

Let's compute term by term:

-2 ln2 + 4 - π²/4

+ (-2 (ln2)^2 + 2 ln2 )

+ (-2 (ln2)^2 + 4 ln2 -4 + π²/6 )

Combine like terms:

-2 ln2 + 2 ln2 + 4 ln2 = 4 ln2

4 -4 = 0

- π²/4 + π²/6 = (-3π²/12 + 2π²/12) = -π²/12

-2 (ln2)^2 -2 (ln2)^2 = -4 (ln2)^2

So total:

4 ln2 -4 (ln2)^2 - π²/12

Therefore, the original integral is equal to 4 ln2 -4 (ln2)^2 - π²/12

Simplify:

Factor out 4:

4( ln2 - (ln2)^2 ) - π²/12

Alternatively, leave as is.

Now, let's compute the numerical value.

First, compute each term:

ln2 ≈ 0.69314718056

(ln2)^2 ≈ (0.69314718056)^2 ≈ 0.480453014

π² ≈ 9.8696044

So:

4 ln2 ≈ 4 * 0.69314718056 ≈ 2.77258872224

4 (ln2)^2 ≈ 4 * 0.480453014 ≈ 1.921812056

π²/12 ≈ 9.8696044 /12 ≈ 0.822467033

So:

4 ln2 -4 (ln2)^2 - π²/12 ≈ 2.77258872224 - 1.921812056 - 0.822467033 ≈

2.77258872224 - 2.744279089 ≈ 0.02830963324

So approximately 0.02830963324

But let's check the calculation again:

Wait, 4 ln2 ≈ 2.77258872224

4 (ln2)^2 ≈ 1.921812056

π²/12 ≈ 0.822467033

So:

2.77258872224 - 1.921812056 = 0.85077666624

Then subtract 0.822467033: 0.85077666624 - 0.822467033 ≈ 0.02830963324

Yes, approximately 0.02830963324, which rounds to 0.0283096332 when rounded to 10 decimal places.

But let's verify this with a more precise calculation.

Alternatively, use exact terms:

The exact answer is 4 ln2 -4 (ln2)^2 - π²/12

But perhaps there's a way to simplify this expression further. Let's see:

Let’s factor out 4:

4( ln2 - (ln2)^2 ) - π²/12

But ln2 - (ln2)^2 = ln2(1 - ln2)

So 4 ln2(1 - ln2) - π²/12

Alternatively, but I don't think this simplifies further. So the exact answer is 4 ln2 -4 (ln2)^2 - π²/12

But let's check if this can be expressed in terms of other constants. Alternatively, it's possible that this expression is the simplest form.

Therefore, the exact answer is:

4 \ln 2 - 4 (\ln 2)^2 - \frac{\pi^2}{12}

And the numerical approximation is approximately 0.0283096332.

But to confirm, let's compute with higher precision:

Compute each term with more decimals:

ln2 ≈ 0.6931471805599453

(ln2)^2 ≈ 0.4804530139182014

π² ≈ 9.869604401089358

So:

4 ln2 = 4 * 0.6931471805599453 ≈ 2.7725887222397812

4 (ln2)^2 = 4 * 0.4804530139182014 ≈ 1.9218120556728056

π²/12 ≈ 9.869604401089358 /12 ≈ 0.8224670334241132

Now, 2.7725887222397812 - 1.9218120556728056 = 0.8507766665669756

Then subtract 0.8224670334241132: 0.8507766665669756 - 0.8224670334241132 ≈ 0.0283096331428624

So approximately 0.0283096331428624, which rounds to 0.0283096331 when rounded to 10 decimal places.

But depending on the exact value, it might be 0.02830963314, which would round to 0.0283096331 or 0.02830963314. Let's check with more precise π²:

π² = 9.869604401089358618... /12 = 0.8224670334241132...

So the subtraction:

0.8507766665669756 - 0.8224670334241132 = 0.0283096331428624

So 0.0283096331428624, which is approximately 0.02830963314 when rounded to 11 decimal places, so to 10 decimal places: 0.02830963314 → 0.0283096331

But let's check with another method. Maybe using numerical integration to verify.

Alternatively, use a calculator to compute the original integral numerically.

But given the exact expression is 4 ln2 -4 (ln2)^2 - π²/12, and the numerical value is approximately 0.0283096331.

Therefore, the final answer is:

Exact: 4 \ln 2 - 4 (\ln 2)^2 - \frac{\pi^2}{12}

Numerical: approximately 0.0283096331

So the JSON output should be:

{"answer": "4\\ln 2 - 4(\\ln 2)^2 - \\frac{\\pi^2}{12}", "numerical_answer": "0.0283096331"}
</think>

{"answer": "4\\ln 2 - 4(\\ln 2)^2 - \\frac{\\pi^2}{12}", "numerical_answer": "0.0283096331"}