<think>
Okay, let's see. I need to compute the definite integral from 0 to 1 of |1 - |1 - |1 - x||| dx. Hmm, that looks a bit complicated with all those absolute value signs. Maybe I should start by simplifying the integrand step by step. 

First, let's break down the innermost absolute value. The expression is |1 - x|. Since x is between 0 and 1, 1 - x is non-negative, right? Because if x is 0, it's 1, and if x is 1, it's 0. So |1 - x| is just 1 - x for x in [0,1]. So that simplifies the inner part.

So replacing the innermost absolute value, the expression becomes |1 - |1 - x|| = |1 - (1 - x)| = |x|. But x is between 0 and 1, so |x| is just x. Therefore, the next layer is |1 - |1 - x|| = x. 

Wait, let me check that. Let me substitute x with some values. For example, if x is 0.5, then |1 - |1 - 0.5|| = |1 - 0.5| = 0.5, which is x. If x is 0.2, same thing: |1 - 0.8| = 0.2. So yes, that seems correct. So the middle absolute value simplifies to x.

Then the outermost absolute value is |1 - x| again? Wait, no. Wait, the original integrand is |1 - |1 - |1 - x|||. We simplified |1 - |1 - x|| to x, so the entire expression becomes |1 - x|. Wait, no. Let me re-express the original integrand step by step.

Original integrand: |1 - |1 - |1 - x|||.

Let me compute the innermost part first: |1 - x|. As established, that's 1 - x for x in [0,1].

Then, the next layer is |1 - |1 - x|| = |1 - (1 - x)| = |x| = x, since x is non-negative.

Then, the outermost absolute value is |1 - x|. Wait, no. Wait, the outermost is |1 - (result of the inner absolute value)|. The inner absolute value was |1 - |1 - x||, which we found to be x. So the entire integrand is |1 - x|. Wait, that can't be right. Wait, let me check again:

Original integrand: |1 - |1 - |1 - x|||.

Let me compute step by step:

Start with |1 - x|. Since x ∈ [0,1], this is 1 - x.

Then, compute |1 - (1 - x)| = |x| = x, since x ≥ 0.

Then, compute |1 - x|. Wait, the outermost absolute value is |1 - (result of the previous step)|. The previous step was x, so |1 - x|. So the integrand simplifies to |1 - x|. But wait, that would mean the entire integrand is |1 - x|, which is the same as the innermost absolute value. But that seems too simple. Let me check with a value. Let's take x = 0.3.

Compute |1 - |1 - |1 - 0.3|||:

First, |1 - 0.3| = 0.7.

Then, |1 - 0.7| = 0.3.

Then, |1 - 0.3| = 0.7. Wait, so the integrand at x=0.3 is 0.7? But if I follow the previous steps, the integrand would be |1 - x|, which is 0.7. So that's correct. Wait, but if x=0.5, then |1 - |1 - |1 - 0.5||| = |1 - |1 - 0.5|| = |1 - 0.5| = 0.5. Wait, but according to the previous steps, the integrand would be |1 - 0.5| = 0.5. So that's the same. Wait, but if x=0.5, the innermost is 0.5, then |1 - 0.5| = 0.5, then |1 - 0.5| = 0.5. So yes, same result. Wait, but if x=0.8, then:

Innermost: |1 - 0.8| = 0.2.

Then |1 - 0.2| = 0.8.

Then |1 - 0.8| = 0.2. Wait, but according to the previous conclusion, the integrand is |1 - x|, which would be 0.2. But here, the actual calculation gives 0.2. Wait, but according to the steps I did earlier, the integrand is |1 - x|. But in this case, when x=0.8, the integrand is 0.2, which is |1 - x|. So maybe the integrand is indeed |1 - x|. But that seems contradictory to the original expression. Wait, let me check again.

Wait, the original integrand is |1 - |1 - |1 - x|||. Let me parse this step by step:

Start with |1 - x|, which is 1 - x for x in [0,1].

Then, compute |1 - (1 - x)| = |x| = x.

Then, compute |1 - x|. Wait, no. Wait, the next layer is |1 - |1 - |1 - x|||. So after computing |1 - |1 - x|| as x, then the entire expression is |1 - x|. Wait, no. Wait, the structure is:

The innermost is |1 - x|. Let's call that A. Then, compute |1 - A|, which is |1 - (1 - x)| = |x| = x. Then, compute |1 - (result of that)|. So |1 - x|. So yes, the integrand is |1 - x|. But that seems like the original integrand is |1 - x|, but the original expression is |1 - |1 - |1 - x|||. So according to this, it's |1 - x|. But that seems like the absolute value is redundant here. Wait, but when I test with x=0.8, the original expression gives 0.2, which is |1 - x|. So maybe the entire integrand simplifies to |1 - x|. But that seems too straightforward. Let me check another value. Let's take x=0. Let's compute the original integrand at x=0:

|1 - |1 - |1 - 0||| = |1 - |1 - 1|| = |1 - 0| = 1. Which is |1 - 0| = 1. So that's 1. Similarly, |1 - x| at x=0 is 1. So that's the same. At x=1, the integrand is |1 - |1 - |1 - 1||| = |1 - |1 - 0|| = |1 - 1| = 0. Which is |1 - 1| = 0. So that's the same. So in all these test cases, the integrand is |1 - x|. Therefore, the integrand simplifies to |1 - x| over [0,1]. Therefore, the integral from 0 to 1 of |1 - x| dx is the same as the integral of (1 - x) dx from 0 to 1, since 1 - x is non-negative there. Wait, but |1 - x| is equal to 1 - x when x ≤ 1, which is always true here. So yes, the integral is ∫₀¹ (1 - x) dx. Then, integrating (1 - x) from 0 to 1 is [x - (x²)/2] from 0 to 1. So at 1, it's 1 - 1/2 = 1/2. At 0, it's 0. So the integral is 1/2. But wait, that seems too easy. The problem is presented as a triple absolute value, but it simplifies to |1 - x|. Is that correct? Let me check again.

Wait, perhaps I made a mistake in the simplification. Let me re-express the original integrand step by step:

Original integrand: |1 - |1 - |1 - x|||.

Let me compute the innermost absolute value first: |1 - x|. Since x ∈ [0,1], this is 1 - x.

Then, the next absolute value is |1 - (1 - x)| = |x| = x, since x is non-negative in [0,1].

Then, the outermost absolute value is |1 - x|. Wait, no. Wait, the outermost is |1 - (result of the previous step)|. The previous step was x, so |1 - x|. Therefore, the integrand is |1 - x|. Therefore, the integrand simplifies to |1 - x|. Therefore, the integral is ∫₀¹ |1 - x| dx. But since 1 - x is non-negative on [0,1], this is ∫₀¹ (1 - x) dx. Which is [x - x²/2] from 0 to 1. Which is (1 - 1/2) - (0 - 0) = 1/2. So the exact answer is 1/2, and the numerical approximation is 0.5. But wait, but the problem is presented as a triple absolute value. Maybe I made a mistake in the simplification. Let me check with another approach.

Alternatively, perhaps the integrand is not |1 - x|. Let me consider the function composition. Let me define f(x) = |1 - |1 - |1 - x|||. Let's analyze f(x) over the interval [0,1].

First, let's consider the innermost function: |1 - x|. As before, this is 1 - x for x ∈ [0,1].

Then, the next layer is |1 - (1 - x)| = |x| = x.

Then, the outermost layer is |1 - x|. So f(x) = |1 - x|. Therefore, the integrand is indeed |1 - x|. Therefore, the integral is 1/2. But that seems too simple. Let me check with x=0.5. f(0.5) = |1 - |1 - |1 - 0.5||| = |1 - |1 - 0.5|| = |1 - 0.5| = 0.5. Which is |1 - 0.5| = 0.5. So yes, same result. Similarly, x=0.25: f(0.25) = |1 - |1 - 0.75|| = |1 - 0.75| = 0.25. Which is |1 - 0.25| = 0.75. Wait, wait, wait. Wait, no. Wait, let's compute step by step for x=0.25:

First, |1 - x| = |1 - 0.25| = 0.75.

Then, |1 - 0.75| = 0.25.

Then, |1 - 0.25| = 0.75. Wait, that's different. Wait, this contradicts the previous conclusion. Wait, so for x=0.25, the original integrand is 0.75, but according to the previous steps, the integrand would be |1 - x| = 0.75. Wait, but according to the step-by-step computation:

Original integrand: |1 - |1 - |1 - x|||.

x=0.25:

1. |1 - x| = 0.75.

2. |1 - 0.75| = 0.25.

3. |1 - 0.25| = 0.75.

So the integrand is 0.75. But according to the previous conclusion that the integrand is |1 - x|, which for x=0.25 is 0.75. So that's the same. Wait, but in this case, the integrand is |1 - x|. So for x=0.25, it's 0.75, which is 1 - x. So yes, same as |1 - x|. Wait, but when x=0.5, the integrand is 0.5, which is |1 - 0.5|. So yes, same. For x=0.75:

1. |1 - 0.75| = 0.25.

2. |1 - 0.25| = 0.75.

3. |1 - 0.75| = 0.25. Wait, wait, no. Wait, step 3 is |1 - (result of step 2)|. Step 2 is 0.75. So step 3 is |1 - 0.75| = 0.25. But according to |1 - x|, when x=0.75, |1 - x| = 0.25. So that's the same. Wait, but in this case, the integrand is 0.25, which is |1 - x|. So yes, the integrand is |1 - x|. So regardless of x, the integrand is |1 - x|. Therefore, the integral is ∫₀¹ |1 - x| dx = ∫₀¹ (1 - x) dx = 1/2. So the answer is 1/2. But wait, but when x=0.75, the integrand is 0.25, which is 1 - x. So yes, the integrand is 1 - x over [0,1]. Therefore, the integral is 1/2. But the problem seems to have a more complex structure. Maybe I made a mistake in the simplification. Let me check another value. Let's take x=0.6.

Original integrand:

1. |1 - 0.6| = 0.4.

2. |1 - 0.4| = 0.6.

3. |1 - 0.6| = 0.4.

Which is |1 - x| = 0.4. So yes, same. So the integrand is indeed |1 - x|. Therefore, the integral is 1/2. So the exact answer is 1/2, and the numerical approximation is 0.5. But I need to make sure that this is correct. Let me think again. Maybe there's a mistake in the step-by-step simplification. Let me write the function as a composition:

Let f(x) = |1 - |1 - |1 - x|||.

Let me define:

Let’s break it down:

Let’s define:

A = |1 - x|

B = |1 - A|

C = |1 - B|

So the integrand is C.

Now, since x ∈ [0,1], A = 1 - x.

Then, B = |1 - (1 - x)| = |x| = x.

Then, C = |1 - B| = |1 - x|.

Therefore, C = |1 - x|. Therefore, the integrand is |1 - x|. Therefore, the integral is ∫₀¹ |1 - x| dx = ∫₀¹ (1 - x) dx = [x - x²/2] from 0 to 1 = (1 - 1/2) - 0 = 1/2. So the exact answer is 1/2, which is 0.5 numerically. Therefore, the answer should be 1/2. But I need to make sure that this is correct. Let me check with a different approach. Maybe graphing the function. If the integrand is |1 - x|, then the graph is a V-shape starting at (0,1) and going down to (1,0). But let's see if the original function is the same. Let's take a few points:

x=0: |1 - |1 - |1 - 0||| = |1 - |1 - 1|| = |1 - 0| = 1. Which matches |1 - 0| = 1.

x=0.5: |1 - |1 - |1 - 0.5||| = |1 - |1 - 0.5|| = |1 - 0.5| = 0.5. Which matches |1 - 0.5| = 0.5.

x=0.75: |1 - |1 - |1 - 0.75||| = |1 - |1 - 0.25|| = |1 - 0.75| = 0.25. Which matches |1 - 0.75| = 0.25.

x=1: |1 - |1 - |1 - 1||| = |1 - |1 - 0|| = |1 - 1| = 0. Which matches |1 - 1| = 0.

So all these points confirm that the integrand is indeed |1 - x|. Therefore, the integral is 1/2. Therefore, the answer is 1/2. So the problem, despite the complex-looking expression, simplifies to a straightforward integral. Therefore, the exact answer is 1/2, and the numerical approximation is 0.5.
</think>

{"answer": "\\frac{1}{2}", "numerical_answer": 0.5000000000}