To solve the definite integral \(\int\limits_{0}^{2} H_{3}\left(\sqrt{x(2-x)}\right) dx\), we need to understand the function \(H_{3}(y)\). The Hermite polynomial \(H_{3}(y)\) is given by:

\[ H_{3}(y) = 8y^3 - 12y \]

Thus, the integral becomes:

\[ \int\limits_{0}^{2} H_{3}\left(\sqrt{x(2-x)}\right) dx = \int\limits_{0}^{2} \left(8\left(\sqrt{x(2-x)}\right)^3 - 12\sqrt{x(2-x)}\right) dx \]

Let's simplify the integrand:

\[ \left(\sqrt{x(2-x)}\right)^3 = \left(x(2-x)\right)^{3/2} \]

So the integral becomes:

\[ \int\limits_{0}^{2} \left(8(x(2-x))^{3/2} - 12\sqrt{x(2-x)}\right) dx \]

We can split this into two separate integrals:

\[ 8 \int\limits_{0}^{2} (x(2-x))^{3/2} dx - 12 \int\limits_{0}^{2} \sqrt{x(2-x)} dx \]

Let's solve each integral separately.

### First Integral: \(\int\limits_{0}^{2} (x(2-x))^{3/2} dx\)

We use the substitution \(u = x(2-x)\). Then \(du = (2 - 2x) dx\), and \(dx = \frac{du}{2(1 - x)}\).

However, this substitution is not straightforward. Instead, we use a trigonometric substitution. Let \(x = 2 \sin^2 \theta\). Then \(dx = 4 \sin \theta \cos \theta d\theta\).

When \(x = 0\), \(\theta = 0\). When \(x = 2\), \(\theta = \frac{\pi}{2}\).

So the integral becomes:

\[ \int\limits_{0}^{\pi/2} (2 \sin^2 \theta (2 - 2 \sin^2 \theta))^{3/2} \cdot 4 \sin \theta \cos \theta d\theta \]

Simplify the integrand:

\[ (2 \sin^2 \theta (2 \cos^2 \theta))^{3/2} = (4 \sin^2 \theta \cos^2 \theta)^{3/2} = 8 \sin^3 \theta \cos^3 \theta \]

So the integral becomes:

\[ 8 \int\limits_{0}^{\pi/2} 8 \sin^3 \theta \cos^3 \theta \cdot 4 \sin \theta \cos \theta d\theta = 256 \int\limits_{0}^{\pi/2} \sin^4 \theta \cos^4 \theta d\theta \]

Using the double-angle identities, we get:

\[ \sin^4 \theta \cos^4 \theta = \left(\frac{\sin 2\theta}{2}\right)^4 = \frac{\sin^4 2\theta}{16} \]

So the integral becomes:

\[ 256 \cdot \frac{1}{16} \int\limits_{0}^{\pi/2} \sin^4 2\theta d\theta = 16 \int\limits_{0}^{\pi/2} \sin^4 2\theta d\theta \]

Using the reduction formula for \(\sin^4 \theta\):

\[ \int \sin^4 \theta d\theta = \frac{3\theta}{8} - \frac{\sin 2\theta}{4} + \frac{\sin 4\theta}{32} + C \]

So:

\[ 16 \int\limits_{0}^{\pi/2} \sin^4 2\theta d\theta = 16 \left[ \frac{3\theta}{8} - \frac{\sin 2\theta}{4} + \frac{\sin 4\theta}{32} \right]_0^{\pi/2} \]

Evaluating this at the limits:

\[ 16 \left[ \frac{3\pi}{16} - 0 + 0 \right] = 16 \cdot \frac{3\pi}{16} = 3\pi \]

### Second Integral: \(\int\limits_{0}^{2} \sqrt{x(2-x)} dx\)

Using the same substitution \(x = 2 \sin^2 \theta\):

\[ \int\limits_{0}^{\pi/2} \sqrt{2 \sin^2 \theta (2 \cos^2 \theta)} \cdot 4 \sin \theta \cos \theta d\theta = 4 \int\limits_{0}^{\pi/2} 2 \sin \theta \cos \theta \cdot 4 \sin \theta \cos \theta d\theta \]

\[ = 8 \int\limits_{0}^{\pi/2} \sin^2 \theta \cos^2 \theta d\theta \]

Using the double-angle identities:

\[ \sin^2 \theta \cos^2 \theta = \left(\frac{\sin 2\theta}{2}\right)^2 = \frac{\sin^2 2\theta}{4} \]

So the integral becomes:

\[ 8 \cdot \frac{1}{4} \int\limits_{0}^{\pi/2} \sin^2 2\theta d\theta = 2 \int\limits_{0}^{\pi/2} \sin^2 2\theta d\theta \]

Using the reduction formula for \(\sin^2 \theta\):

\[ \int \sin^2 \theta d\theta = \frac{\theta}{2} - \frac{\sin 2\theta}{4} + C \]

So:

\[ 2 \int\limits_{0}^{\pi/2} \sin^2 2\theta d\theta = 2 \left[ \frac{\theta}{2} - \frac{\sin 2\theta}{4} \right]_0^{\pi/2} \]

Evaluating this at the limits:

\[ 2 \left[ \frac{\pi}{4} - 0 \right] = 2 \cdot \frac{\pi}{4} = \frac{\pi}{2} \]

### Combining the Results

\[ 8 \cdot 3\pi - 12 \cdot \frac{\pi}{2} = 24\pi - 6\pi = 18\pi \]

### Numerical Approximation

\[ 18\pi \approx 56.54867316 \]

### Final Answer

```json
{"answer": "18\\pi", "numerical_answer": "56.54867316"}
```