To solve the definite integral \(\int_{0}^{1} x^{-1/2}(1-x)^{-1/2} T_{4}\left(\sqrt{x(1-x)}\right) \, dx\), we need to carefully analyze the integrand and use appropriate techniques.

### Step 1: Analyze the Integrand

The integrand is \(x^{-1/2}(1-x)^{-1/2} T_{4}\left(\sqrt{x(1-x)}\right)\), where \(T_{4}(y)\) is the Chebyshev polynomial of the first kind of degree 4. The Chebyshev polynomial \(T_{4}(y)\) is given by:
\[ T_{4}(y) = 8y^4 - 8y^2 + 1. \]

Substituting \(y = \sqrt{x(1-x)}\), we get:
\[ T_{4}\left(\sqrt{x(1-x)}\right) = 8(x(1-x))^2 - 8(x(1-x)) + 1. \]

### Step 2: Simplify the Integrand

Let's simplify the expression inside the integral:
\[ T_{4}\left(\sqrt{x(1-x)}\right) = 8(x(1-x))^2 - 8(x(1-x)) + 1. \]

Expanding \((x(1-x))^2\):
\[ (x(1-x))^2 = x^2(1 - 2x + x^2) = x^2 - 2x^3 + x^4. \]

Thus,
\[ T_{4}\left(\sqrt{x(1-x)}\right) = 8(x^2 - 2x^3 + x^4) - 8(x - x^2) + 1. \]

Simplifying further:
\[ T_{4}\left(\sqrt{x(1-x)}\right) = 8x^2 - 16x^3 + 8x^4 - 8x + 8x^2 + 1. \]
\[ T_{4}\left(\sqrt{x(1-x)}\right) = 8x^4 - 16x^3 + 16x^2 - 8x + 1. \]

### Step 3: Set Up the Integral

Now, the integral becomes:
\[ \int_{0}^{1} x^{-1/2}(1-x)^{-1/2} (8x^4 - 16x^3 + 16x^2 - 8x + 1) \, dx. \]

We can split this into separate integrals:
\[ 8 \int_{0}^{1} x^{7/2}(1-x)^{-1/2} \, dx - 16 \int_{0}^{1} x^{5/2}(1-x)^{-1/2} \, dx + 16 \int_{0}^{1} x^{3/2}(1-x)^{-1/2} \, dx - 8 \int_{0}^{1} x^{1/2}(1-x)^{-1/2} \, dx + \int_{0}^{1} x^{-1/2}(1-x)^{-1/2} \, dx. \]

### Step 4: Evaluate Each Integral

Each of these integrals is of the form \(\int_{0}^{1} x^{a}(1-x)^{b} \, dx\), which is a Beta function \(B(a+1, b+1)\). The Beta function is related to the Gamma function by:
\[ B(a+1, b+1) = \frac{\Gamma(a+1)\Gamma(b+1)}{\Gamma(a+b+2)}. \]

For \(a = -1/2\) and \(b = -1/2\):
\[ \int_{0}^{1} x^{-1/2}(1-x)^{-1/2} \, dx = B\left(\frac{1}{2}, \frac{1}{2}\right) = \frac{\Gamma\left(\frac{1}{2}\right)\Gamma\left(\frac{1}{2}\right)}{\Gamma(1)} = \pi. \]

For \(a = 1/2\) and \(b = -1/2\):
\[ \int_{0}^{1} x^{1/2}(1-x)^{-1/2} \, dx = B\left(\frac{3}{2}, \frac{1}{2}\right) = \frac{\Gamma\left(\frac{3}{2}\right)\Gamma\left(\frac{1}{2}\right)}{\Gamma(2)} = \frac{\sqrt{\pi} \cdot \sqrt{\pi}}{2} = \frac{\pi}{2}. \]

For \(a = 3/2\) and \(b = -1/2\):
\[ \int_{0}^{1} x^{3/2}(1-x)^{-1/2} \, dx = B\left(\frac{5}{2}, \frac{1}{2}\right) = \frac{\Gamma\left(\frac{5}{2}\right)\Gamma\left(\frac{1}{2}\right)}{\Gamma(3)} = \frac{\frac{3}{2}\sqrt{\pi} \cdot \sqrt{\pi}}{2} = \frac{3\pi}{4}. \]

For \(a = 5/2\) and \(b = -1/2\):
\[ \int_{0}^{1} x^{5/2}(1-x)^{-1/2} \, dx = B\left(\frac{7}{2}, \frac{1}{2}\right) = \frac{\Gamma\left(\frac{7}{2}\right)\Gamma\left(\frac{1}{2}\right)}{\Gamma(4)} = \frac{\frac{15}{8}\sqrt{\pi} \cdot \sqrt{\pi}}{6} = \frac{15\pi}{16}. \]

For \(a = 7/2\) and \(b = -1/2\):
\[ \int_{0}^{1} x^{7/2}(1-x)^{-1/2} \, dx = B\left(\frac{9}{2}, \frac{1}{2}\right) = \frac{\Gamma\left(\frac{9}{2}\right)\Gamma\left(\frac{1}{2}\right)}{\Gamma(5)} = \frac{\frac{105}{16}\sqrt{\pi} \cdot \sqrt{\pi}}{24} = \frac{105\pi}{384}. \]

### Step 5: Combine the Results

Combining all the results:
\[ 8 \cdot \frac{105\pi}{384} - 16 \cdot \frac{15\pi}{16} + 16 \cdot \frac{3\pi}{4} - 8 \cdot \frac{\pi}{2} + \pi. \]

Simplifying each term:
\[ 8 \cdot \frac{105\pi}{384} = \frac{840\pi}{384} = \frac{35\pi}{16}, \]
\[ -16 \cdot \frac{15\pi}{16} = -15\pi, \]
\[ 16 \cdot \frac{3\pi}{4} = 12\pi, \]
\[ -8 \cdot \frac{\pi}{2} = -4\pi, \]
\[ + \pi. \]

Combining these:
\[ \frac{35\pi}{16} - 15\pi + 12\pi - 4\pi + \pi = \frac{35\pi}{16} - 6\pi. \]

Converting \(-6\pi\) to a fraction with denominator 16:
\[ -6\pi = -\frac{96\pi}{16}. \]

Thus:
\[ \frac{35\pi}{16} - \frac{96\pi}{16} = -\frac{61\pi}{16}. \]

### Step 6: Numerical Approximation

The numerical approximation of \(-\frac{61\pi}{16}\) is:
\[ -\frac{61\pi}{16} \approx -12.094757057. \]

### Final Answer

The final answer in the required JSON format is:
```json
{"answer": "-\\frac{61\\pi}{16}", "numerical_answer": "-12.094757057"}
```