To solve the definite integral 

\[
\int_{\frac{1}{8}}^{\frac{1}{4}} \frac{\ln(2x)\ln(4x)\ln(8x)}{x} \, dx,
\]

we proceed with the following steps:

### Step 1: Simplify the Integrand
First, express the logarithms in terms of \(\ln x\):

\[
\ln(2x) = \ln 2 + \ln x,
\]
\[
\ln(4x) = \ln 4 + \ln x = 2\ln 2 + \ln x,
\]
\[
\ln(8x) = \ln 8 + \ln x = 3\ln 2 + \ln x.
\]

Let \( u = \ln x \). Then, \( du = \frac{1}{x} dx \). The integral becomes:

\[
\int (\ln 2 + u)(2\ln 2 + u)(3\ln 2 + u) \, du.
\]

### Step 2: Expand the Integrand
Expand the product:

\[
(\ln 2 + u)(2\ln 2 + u)(3\ln 2 + u).
\]

First, multiply the first two factors:

\[
(\ln 2 + u)(2\ln 2 + u) = 2(\ln 2)^2 + 3\ln 2 \cdot u + u^2.
\]

Now, multiply by the third factor:

\[
(2(\ln 2)^2 + 3\ln 2 \cdot u + u^2)(3\ln 2 + u) = 6(\ln 2)^3 + 11(\ln 2)^2 u + 6\ln 2 \cdot u^2 + u^3.
\]

### Step 3: Integrate Term by Term
Integrate with respect to \( u \):

\[
\int \left(6(\ln 2)^3 + 11(\ln 2)^2 u + 6\ln 2 \cdot u^2 + u^3\right) du = 6(\ln 2)^3 u + \frac{11}{2}(\ln 2)^2 u^2 + 2\ln 2 \cdot u^3 + \frac{1}{4}u^4 + C.
\]

### Step 4: Apply the Limits of Integration
The limits for \( u \) are:

\[
\text{When } x = \frac{1}{8}, \quad u = \ln\left(\frac{1}{8}\right) = -\ln 8 = -3\ln 2.
\]
\[
\text{When } x = \frac{1}{4}, \quad u = \ln\left(\frac{1}{4}\right) = -\ln 4 = -2\ln 2.
\]

Evaluate the antiderivative at these limits:

\[
\left[6(\ln 2)^3 u + \frac{11}{2}(\ln 2)^2 u^2 + 2\ln 2 \cdot u^3 + \frac{1}{4}u^4\right]_{-3\ln 2}^{-2\ln 2}.
\]

Compute each term at \( u = -2\ln 2 \) and \( u = -3\ln 2 \):

At \( u = -2\ln 2 \):

\[
6(\ln 2)^3 (-2\ln 2) = -12(\ln 2)^4,
\]
\[
\frac{11}{2}(\ln 2)^2 (-2\ln 2)^2 = \frac{11}{2}(\ln 2)^2 \cdot 4(\ln 2)^2 = 22(\ln 2)^4,
\]
\[
2\ln 2 \cdot (-2\ln 2)^3 = 2\ln 2 \cdot (-8)(\ln 2)^3 = -16(\ln 2)^4,
\]
\[
\frac{1}{4}(-2\ln 2)^4 = \frac{1}{4} \cdot 16(\ln 2)^4 = 4(\ln 2)^4.
\]

Summing these:

\[
-12(\ln 2)^4 + 22(\ln 2)^4 - 16(\ln 2)^4 + 4(\ln 2)^4 = -2(\ln 2)^4.
\]

At \( u = -3\ln 2 \):

\[
6(\ln 2)^3 (-3\ln 2) = -18(\ln 2)^4,
\]
\[
\frac{11}{2}(\ln 2)^2 (-3\ln 2)^2 = \frac{11}{2}(\ln 2)^2 \cdot 9(\ln 2)^2 = \frac{99}{2}(\ln 2)^4,
\]
\[
2\ln 2 \cdot (-3\ln 2)^3 = 2\ln 2 \cdot (-27)(\ln 2)^3 = -54(\ln 2)^4,
\]
\[
\frac{1}{4}(-3\ln 2)^4 = \frac{1}{4} \cdot 81(\ln 2)^4 = \frac{81}{4}(\ln 2)^4.
\]

Summing these:

\[
-18(\ln 2)^4 + \frac{99}{2}(\ln 2)^4 - 54(\ln 2)^4 + \frac{81}{4}(\ln 2)^4 = \left(-18 + \frac{99}{2} - 54 + \frac{81}{4}\right)(\ln 2)^4.
\]

Convert to a common denominator (4):

\[
\left(-\frac{72}{4} + \frac{198}{4} - \frac{216}{4} + \frac{81}{4}\right)(\ln 2)^4 = \left(-\frac{72 + 216}{4} + \frac{198 + 81}{4}\right)(\ln 2)^4 = \left(-\frac{288}{4} + \frac{279}{4}\right)(\ln 2)^4 = -\frac{9}{4}(\ln 2)^4.
\]

### Step 5: Subtract the Lower Limit from the Upper Limit
\[
\text{Integral} = \left(-2(\ln 2)^4\right) - \left(-\frac{9}{4}(\ln 2)^4\right) = \left(-2 + \frac{9}{4}\right)(\ln 2)^4 = \frac{1}{4}(\ln 2)^4.
\]

### Step 6: Numerical Approximation
Using \(\ln 2 \approx 0.6931471806\):

\[
\frac{1}{4}(\ln 2)^4 \approx \frac{1}{4}(0.6931471806)^4 \approx \frac{1}{4} \times 0.2302585093 \approx 0.0575646273.
\]

### Final Answer
\[
\boxed{\frac{(\ln 2)^4}{4}}
\]

Numerical approximation: \(0.0575646273\).

```json
{"answer": "\\frac{(\\ln 2)^4}{4}", "numerical_answer": "0.0575646273"}
```