Let’s consider the integral:
\[
I = \int_0^{2\pi} \tan(\cos x)\,dx
\]

**Step 1: Symmetry Analysis**

Notice that
\[
\tan(\cos(2\pi-x)) = \tan(\cos x)
\]
because \(\cos(2\pi - x) = \cos x\).

This means the function is periodic and symmetric over \([0, 2\pi]\).

Let’s consider the function \(f(x) = \tan(\cos x)\). Let's check if it's odd/even about \(x = \pi\):
\[
\cos(\pi + t) = -\cos t
\]
So, let’s make the substitution \(x = \pi + t\), where as \(x\) goes from \(0\) to \(2\pi\), \(t\) goes from \(-\pi\) to \(\pi\):

Let’s split the integral:
\[
I = \int_0^{2\pi} \tan(\cos x)\,dx = \int_0^{\pi} \tan(\cos x)\,dx + \int_{\pi}^{2\pi} \tan(\cos x)\,dx
\]

In the second integral, let \(u = x - \pi\), so as \(x\) goes from \(\pi\) to \(2\pi\), \(u\) goes from \(0\) to \(\pi\):
\[
\int_{\pi}^{2\pi} \tan(\cos x)\,dx = \int_0^{\pi} \tan(\cos(u+\pi))\,du
\]
But \(\cos(u+\pi) = -\cos u\), so
\[
\tan(\cos(u+\pi)) = \tan(-\cos u) = -\tan(\cos u)
\]
Therefore,
\[
I = \int_0^{\pi} \tan(\cos x)\,dx + \int_0^{\pi} [-\tan(\cos u)]\,du = \int_0^{\pi} \tan(\cos x)\,dx - \int_0^{\pi} \tan(\cos x)\,dx = 0
\]
So the integral evaluates to 0.

**Step 2: Final Exact And Numerical Answers**

Exact answer: \(0\)

Numerical approximation: \(0.0000000000\)

**Step 3: JSON Output**

```json
{"answer": "0", "numerical_answer": "0.0000000000"}
```