Let's analyze the integral:
\[
I = \int_0^{\frac{\pi}{4}} \ln(\cot x - 1)\,dx
\]

### Step 1: Simplify the Integrand

First, recall that:
\[
\cot x - 1 = \frac{\cos x}{\sin x} - 1 = \frac{\cos x - \sin x}{\sin x}
\]
So,
\[
\ln(\cot x - 1) = \ln(\cos x - \sin x) - \ln(\sin x)
\]
Thus,
\[
I = \int_0^{\frac{\pi}{4}} \ln(\cos x - \sin x)\,dx - \int_0^{\frac{\pi}{4}} \ln(\sin x)\,dx
\]

#### 1.1 Simplifying \(\cos x - \sin x\)
\[
\cos x - \sin x = \sqrt{2} \left( \frac{1}{\sqrt{2}} \cos x - \frac{1}{\sqrt{2}} \sin x \right)
= \sqrt{2}\left( \cos\frac{\pi}{4} \cos x - \sin\frac{\pi}{4} \sin x \right)
\]
\[
= \sqrt{2} \cos\left(x + \frac{\pi}{4}\right)
\]
Thus,
\[
\ln(\cos x - \sin x) = \frac{1}{2} \ln 2 + \ln\left( \cos\left( x + \frac{\pi}{4} \right)\right)
\]

So,
\[
I = \int_0^{\frac{\pi}{4}} \left[\frac{1}{2}\ln 2 + \ln\left(\cos\left(x+\frac{\pi}{4}\right)\right) - \ln \sin x \right] dx
\]
\[
= \int_0^{\frac{\pi}{4}} \left( \frac{1}{2}\ln 2 \right) dx + \int_0^{\frac{\pi}{4}}\ln\left(\cos\left(x+\frac{\pi}{4}\right)\right) dx - \int_0^{\frac{\pi}{4}}\ln\sin x dx
\]
\[
= \frac{\pi}{8}\ln 2 + \int_0^{\frac{\pi}{4}}\ln\left(\cos\left(x+\frac{\pi}{4}\right)\right) dx - \int_0^{\frac{\pi}{4}}\ln\sin x dx
\]

### Step 2: Further Simplify and Change of Variables

Focus on the second integral. Let \( u = x + \frac{\pi}{4} \implies x = u - \frac{\pi}{4} \).
When \( x = 0, u = \frac{\pi}{4} \)
When \( x = \frac{\pi}{4}, u = \frac{\pi}{2} \)

So,
\[
\int_0^{\frac{\pi}{4}} \ln\left(\cos\left(x+\frac{\pi}{4}\right)\right)\,dx
= \int_{\frac{\pi}{4}}^{\frac{\pi}{2}} \ln(\cos u)\,du
\]

So, we update:
\[
I = \frac{\pi}{8}\ln 2 + \int_{\frac{\pi}{4}}^{\frac{\pi}{2}} \ln(\cos u)\,du - \int_0^{\frac{\pi}{4}} \ln(\sin x)\,dx
\]

### Step 3: Use Logarithm of Sine and Cosine Integrals

Define the **log-sine integral:**
\[
S(a) = \int_0^a \ln(\sin x)\, dx
\]
and the **log-cosine integral:**
\[
C(a) = \int_0^a \ln(\cos x)\, dx
\]

Thus, our integral is:
\[
I = \frac{\pi}{8}\ln 2 + [C(\frac{\pi}{2}) - C(\frac{\pi}{4})] - S(\frac{\pi}{4})
\]

It is known that:
\[
C\left(\frac{\pi}{2}\right) = \int_0^{\frac{\pi}{2}}\ln(\cos x)\,dx = -\frac{\pi}{2}\ln 2
\]

### Step 4: Express Everything in Terms of Log-Sine

But we can relate \( C(a) \) and \( S(a) \) via symmetries:
\[
C(a) = S(a) + \ln 2\,a - S\left(\frac{\pi}{2} - a\right)
\]
But what we have is more direct with tabulated values.

We already have:
\[
J = \int_0^{\frac{\pi}{4}} \ln(\sin x)\,dx = S\left(\frac{\pi}{4}\right)
\]
and
\[
K = \int_0^{\frac{\pi}{4}} \ln(\cos x)\,dx
\]

But we need \( C(\frac{\pi}{4}) = K \).

### Step 5: Substitute to Isolate Standard Quantities

Thus:
\[
I = \frac{\pi}{8}\ln 2 - C\left( \frac{\pi}{4} \right) + C\left( \frac{\pi}{2} \right) - S\left( \frac{\pi}{4} \right)
\]
But \( C(\frac{\pi}{4}) = K \).

So:
\[
I = \frac{\pi}{8} \ln 2 + C\left(\frac{\pi}{2}\right) - K - S\left(\frac{\pi}{4}\right)
\]

Since \( C(\frac{\pi}{2}) = -\frac{\pi}{2} \ln 2 \):
\[
I = \frac{\pi}{8} \ln 2 - \frac{\pi}{2}\ln 2 - K - S\left( \frac{\pi}{4} \right)
\]
\[
I = \left( \frac{1}{8} - \frac{1}{2} \right)\pi \ln 2 - K - S\left( \frac{\pi}{4} \right)
\]
\[
I = -\frac{3\pi}{8}\ln 2 - K - S\left( \frac{\pi}{4} \right)
\]

But notice:
\[
K = \int_0^{\frac{\pi}{4}}\ln(\cos x)\, dx
\]
\[
S\left( \frac{\pi}{4} \right ) = \int_0^{\frac{\pi}{4}}\ln (\sin x)\, dx
\]

### Step 6: Find \( K + S(\frac{\pi}{4}) \)

It is a classic calculation that:
\[
\int_0^a \ln(\sin x)\, dx + \int_0^a \ln(\cos x)\, dx = -a \ln 2 + \int_0^a \ln(\sin 2x)\, dx
\]

For \( a = \frac{\pi}{4} \), \( \sin 2a = \sin(\frac{\pi}{2}) = 1 \):

\[
K + S\left( \frac{\pi}{4} \right ) = -\frac{\pi}{4}\ln 2 + \int_0^{\frac{\pi}{4}}\ln (\sin 2x)\, dx
\]

Now, \( \int_0^{\frac{\pi}{4}} \ln (\sin 2x)\, dx \):

Letâ€™s substitute \( t = 2x \),
When \( x=0 \), \( t=0 \),
When \( x=\frac{\pi}{4} \), \( t = \frac{\pi}{2} \),
\( dx = dt/2 \),
So,

\[
\int_0^{\frac{\pi}{4}} \ln (\sin 2x)\, dx = \frac{1}{2} \int_0^{\frac{\pi}{2}} \ln (\sin t)\, dt
\]

And a well-known result:
\[
\int_0^{\frac{\pi}{2}} \ln (\sin t)\, dt = -\frac{\pi}{2} \ln 2 
\]

Therefore:
\[
\int_0^{\frac{\pi}{4}} \ln (\sin 2x) dx = \frac{1}{2} \left( -\frac{\pi}{2} \ln 2 \right ) = -\frac{\pi}{4} \ln 2
\]

So,
\[
K + S\left(\frac{\pi}{4}\right ) = -\frac{\pi}{4}\ln 2 -\frac{\pi}{4}\ln 2 = -\frac{\pi}{2} \ln 2
\]

### Step 7: Compute the Final Value

Recall:
\[
I = -\frac{3\pi}{8}\ln 2 - [K + S(\frac{\pi}{4})] = -\frac{3\pi}{8}\ln 2 - \left ( -\frac{\pi}{2}\ln 2 \right ) 
\]
\[
= -\frac{3\pi}{8}\ln 2 + \frac{\pi}{2}\ln 2
= \left( \frac{1}{2} - \frac{3}{8} \right)\pi \ln 2
= \frac{1}{8}\pi \ln 2
\]

### Step 8: Give the Final Answers

#### Exact Answer:
\[
\boxed{I = \frac{1}{8}\pi \ln 2}
\]

#### Numerical Approximation:

\[
\frac{\pi}{8} \ln 2 \approx \frac{3.141592653589793}{8} \times 0.6931471805599453 \approx 0.3926990817 \times 0.6931471806 \approx 0.2727807844
\]

### Step 9: JSON Output

```json
{"answer": "\\frac{1}{8}\\pi \\ln 2", "numerical_answer": "0.2727807844"}
```