Let's compute the integral
\[
I = \int_0^\infty \frac{\sin(\sqrt{3}x) - \sin\left(\frac{x}{\sqrt{3}}\right)}{x} e^{-x^2} \, dx
\]

**Step 1: Split the Integral**

Let’s denote:
\[
I = I_1 - I_2
\]
with
\[
I_1 = \int_0^\infty \frac{\sin(\sqrt{3}x)}{x} e^{-x^2} dx
\]
\[
I_2 = \int_0^\infty \frac{\sin(x/\sqrt{3})}{x} e^{-x^2} dx
\]

**Step 2: General Formula**

Recall the known result:
\[
\int_0^\infty \frac{\sin(ax)}{x} e^{-b x^2}\, dx = \frac{\pi}{2} \operatorname{erf}\left(\frac{a}{2\sqrt{b}}\right), \quad a > 0,\, b > 0
\]
(See, e.g., Gradshteyn & Ryzhik 3.944.4.)

Here \( b = 1 \), so:
\[
\int_0^\infty \frac{\sin(ax)}{x} e^{-x^2} dx = \frac{\pi}{2} \operatorname{erf}\left(\frac{a}{2}\right)
\]

Therefore,
\[
I_1 = \frac{\pi}{2} \operatorname{erf}\left(\frac{\sqrt{3}}{2}\right)
\]
\[
I_2 = \frac{\pi}{2} \operatorname{erf}\left(\frac{1}{2\sqrt{3}}\right)
\]

Thus,
\[
I = \frac{\pi}{2} \left[ \operatorname{erf}\left(\frac{\sqrt{3}}{2}\right) - \operatorname{erf}\left(\frac{1}{2\sqrt{3}}\right) \right]
\]

**Step 3: Numerical Evaluation**

Let’s calculate the two arguments:
- \( a_1 = \frac{\sqrt{3}}{2} \approx 0.8660254038 \)
- \( a_2 = \frac{1}{2\sqrt{3}} \approx 0.2886751346 \)

Compute the error functions:
- \( \operatorname{erf}(0.8660254038) \approx 0.7989809180 \)
- \( \operatorname{erf}(0.2886751346) \approx 0.3162361176 \)

Take the difference:
- Difference: \( 0.7989809180 - 0.3162361176 = 0.4827448004 \)

Multiply by \( \frac{\pi}{2} \):
- \( \frac{\pi}{2} \approx 1.5707963268 \)
- Final: \( 1.5707963268 \times 0.4827448004 \approx 0.7588355278 \)

**Step 4: Format the Answer**

JSON output:
```json
{"answer": "\\frac{\\pi}{2} \\left[ \\operatorname{erf}\\left( \\frac{\\sqrt{3}}{2} \\right ) - \\operatorname{erf}\\left( \\frac{1}{2\\sqrt{3}} \\right) \\right]", "numerical_answer": "0.7588355278"}
```