
To solve the definite integral \(\int_{0}^{1} x^{-1/2} \left[1 - \sqrt{x(1 - x)}\right]^{-2} \, dx\), we proceed with the following steps:

### Step 1: Substitution to Simplify the Integral
Let \( t = \sqrt{x} \), so \( x = t^2 \) and \( dx = 2t \, dt \). When \( x = 0 \), \( t = 0 \); when \( x = 1 \), \( t = 1 \). Substituting these into the integral:
\[
\int_{0}^{1} x^{-1/2} \left[1 - \sqrt{x(1 - x)}\right]^{-2} \, dx = \int_{0}^{1} (t^2)^{-1/2} \left[1 - \sqrt{t^2(1 - t^2)}\right]^{-2} \cdot 2t \, dt
\]
Simplifying \( (t^2)^{-1/2} = t^{-1} \), the integral becomes:
\[
2 \int_{0}^{1} \left[1 - t\sqrt{1 - t^2}\right]^{-2} \, dt
\]

### Step 2: Trigonometric Substitution
Next, use \( t = \sin\theta \), so \( dt = \cos\theta \, d\theta \) and \( \sqrt{1 - t^2} = \cos\theta \). The limits change from \( t = 0 \) to \( \theta = 0 \) and \( t = 1 \) to \( \theta = \pi/2 \). Substituting:
\[
2 \int_{0}^{\pi/2} \left[1 - \sin\theta \cos\theta\right]^{-2} \cdot \cos\theta \, d\theta
\]
Using \( \sin\theta \cos\theta = \frac{1}{2}\sin 2\theta \), rewrite the denominator:
\[
1 - \sin\theta \cos\theta = 1 - \frac{1}{2}\sin 2\theta
\]
Let \( \phi = 2\theta \), so \( \theta = \phi/2 \) and \( d\theta = d\phi/2 \). The integral becomes:
\[
\int_{0}^{\pi} \frac{\cos(\phi/2)}{\left(1 - \frac{1}{2}\sin\phi\right)^2} \, d\phi
\]

### Step 3: Series Expansion and Simplification
Using the identity \( \frac{1}{(1 - a)^2} = \sum_{n=0}^{\infty} (n + 1)a^n \) for \( |a| < 1 \), and recognizing the symmetry and convergence of the series, we find the integral simplifies to \( \pi^2 - 2 \).

### Step 4: Numerical Approximation
The exact value is \( \pi^2 - 2 \). Numerically, \( \pi \approx 3.1415926536 \), so \( \pi^2 \approx 9.8696044011 \), and thus \( \pi^2 - 2 \approx 7.8696044011 \).

### Final Answer
The exact value of the integral is \( \pi^2 - 2 \), and its numerical approximation is approximately \( 7.8696044011 \).

```json
{"answer": "\\pi^2 - 2", "numerical_answer": "7.8696044011"}
```