Let's proceed step by step.

We are to compute:
\[
I = \int_0^1 \left| 1 - \left| 1 - \left| 1 - x \right| \right| \right| dx
\]

### Step 1: Simplify the Expression

Let us work inside-out.

#### 1. Compute \(|1-x|\):

- For \(0 \leq x \leq 1\), \(1-x\) runs from 1 to 0, and is always non-negative. So \(|1-x| = 1-x\).

Thus,
\[
|1-x| = 1-x\quad\text{for } x \in [0,1]
\]

#### 2. Next level: \(|1 - |1-x||\):

So
\[
|1 - |1-x|| = |1 - (1-x)| = |x| = x
\]
for \(x\in[0,1]\).

#### 3. Outer layer: \(1 - |1 - |1-x|||\):

\[
|1 - |1 - |1-x|| | 
\]
We already have \(|1 - |1-x|| = x\).
So now:
\[
|1-x| \to 1-x;\quad |1 - (1-x)| \to x;\quad |1-x| \in [0,1]
\]
So \(x\in[0,1]\).

So,
\[
|1 - |1 - |1-x|| | = |1 - x|
\]
But, \(x \in [0,1]\), so \(1-x \ge0\). Hence,
\[
|1 - x| = 1 - x
\]

### Step 2: Substitute into the Integral

So,
\[
I = \int_0^1 |1 - |1 - |1-x|| | dx = \int_0^1 (1-x)\; dx
\]

### Step 3: Compute the Integral

\[
\int_0^1 (1-x) dx = \left[ x - \frac{x^2}{2} \right]_0^1 = (1 - \frac{1}{2}) - (0 - 0) = \frac{1}{2}
\]

### Step 4: Numerical Approximation

\[
\frac{1}{2} = 0.5
\]

Rounded to ten decimal places:
\[
0.5000000000
\]

### Step 5: Output in JSON Format

```json
{"answer": "\\frac{1}{2}", "numerical_answer": "0.5000000000"}
```