

To solve the definite integral \(\int_{420}^{1672}\frac{\sqrt{\ln(2023-x)}}{\sqrt{\ln(2023-x)}+\sqrt{\ln(x-69)}}\:\mathrm{d}x\), we use a symmetry substitution.

### Step 1: Substitution
Let \( t = 2092 - x \) (where \( 2092 = 420 + 1672 \), the sum of the limits of integration). This substitution reverses the limits of integration and transforms the integrand. 

- When \( x = 420 \), \( t = 2092 - 420 = 1672 \).
- When \( x = 1672 \), \( t = 2092 - 1672 = 420 \).
- The differential \( \mathrm{d}t = -\mathrm{d}x \), so \( \mathrm{d}x = -\mathrm{d}t \).

### Step 2: Transform the Integrand
Under the substitution \( t = 2092 - x \), we analyze the arguments of the logarithms:
- \( 2023 - x = 2023 - (2092 - t) = t - 69 \),
- \( x - 69 = (2092 - t) - 69 = 2023 - t \).

Thus, the integrand becomes:
\[
\frac{\sqrt{\ln(2023 - x)}}{\sqrt{\ln(2023 - x)} + \sqrt{\ln(x - 69)}} \implies \frac{\sqrt{\ln(t - 69)}}{\sqrt{\ln(t - 69)} + \sqrt{\ln(2023 - t)}}.
\]

### Step 3: Relate the Original and Substituted Integrals
Let \( I \) denote the original integral. The substituted integral (after reversing limits and absorbing the negative sign) is:
\[
I = \int_{420}^{1672} \frac{\sqrt{\ln(t - 69)}}{\sqrt{\ln(t - 69)} + \sqrt{\ln(2023 - t)}} \:\mathrm{d}t.
\]

Notice that the original integrand \( f(x) \) and the substituted integrand \( f(t) \) satisfy \( f(x) + f(t) = 1 \), because:
\[
\frac{\sqrt{\ln(2023 - x)}}{\sqrt{\ln(2023 - x)} + \sqrt{\ln(x - 69)}} + \frac{\sqrt{\ln(x - 69)}}{\sqrt{\ln(2023 - x)} + \sqrt{\ln(x - 69)}} = 1.
\]

### Step 4: Solve for \( I \)
Adding the original integral \( I \) and the substituted integral \( I \), we get:
\[
I + I = \int_{420}^{1672} 1 \:\mathrm{d}x.
\]
Thus, \( 2I = 1672 - 420 \), so \( I = \frac{1672 - 420}{2} = 626 \).

### Numerical Approximation
The exact value is \( 626 \), so the numerical approximation (rounded to 10 decimal places) is \( 626.0000000000 \).

{"answer": "626", "numerical_answer": "626.0000000000"}