We wish to evaluate

  I = ∫₁∞ x (x² – 1)^(2–3/2) e^(–0.5² x²) H₍₂*₂₎(0.5 x) dx.

Step 1. Rewrite the integrand.

• Note that 2 – 3/2 = 1/2 so
  (x²–1.0²)^(2–3/2) = √(x²–1).

• Also, 0.5² = 0.25 so e^(–0.5² x²) = e^(–x²/4).

• The Hermite polynomial H₍₂*₂₎(0.5x) is H₄(0.5x). Recall that
  H₄(z) = 16 z⁴ – 48 z² + 12.
Substitute z = 0.5x:
  H₄(0.5x) = 16 (0.5x)⁴ – 48 (0.5x)² + 12
        = 16 (x⁴/16) – 48 (x²/4) + 12
        = x⁴ – 12x² + 12.

Thus the integrand becomes:
  x · √(x²–1) · e^(–x²/4) · (x⁴ – 12x² + 12)
     = e^(–x²/4) √(x²–1) (x⁵ – 12x³ + 12x).

So we now have
  I = ∫₁∞ e^(–x²/4) √(x²–1) (x⁵ – 12x³ + 12x) dx.

Step 2. Use a substitution to reduce the integral.

A good change is to let u = x². Then:
  du/dx = 2x ⟹ x dx = du/2.
Also, √(x²–1) = √(u–1) and
  x⁵ – 12x³ + 12x = x (x⁴ – 12x² + 12) = x ((x²)² – 12x² + 12).
Since x² = u, we have
  x⁴ – 12x² + 12 = u² – 12u + 12.
Thus the integrand times dx becomes:
  e^(–u/4) √(u–1) [x (u² – 12u + 12)] dx = e^(–u/4) √(u–1) (u² – 12u + 12) (du/2).

The limits change: when x = 1, u = 1; when x → ∞, u → ∞.

So
  I = (1/2) ∫₁∞ e^(–u/4) (u² – 12u + 12) √(u–1) du.

Now let v = u – 1 so that u = v + 1 and du = dv. When u = 1, v = 0; when u → ∞, v → ∞. Also,
  √(u–1) = √v  and
  u² – 12u + 12 = (v+1)² – 12(v+1) + 12.
Expand:
  (v² + 2v + 1) – 12v – 12 + 12 = v² – 10v + 1.
Thus,
  I = (1/2) e^(–1/4) ∫₀∞ e^(–v/4) (v² – 10v + 1) √v dv.

Step 3. Express the integral in terms of Gamma functions.

Write √v = v^(1/2) so that the integrals break into standard forms:
  I = (e^(–1/4)/(2)) { ∫₀∞ e^(–v/4) v^(5/2) dv – 10 ∫₀∞ e^(–v/4) v^(3/2) dv + ∫₀∞ e^(–v/4) v^(1/2) dv }.

Recall the formula:
  ∫₀∞ e^(–v/λ) v^(s–1) dv = Γ(s) λ^s  (for λ > 0).

Here, with λ = 4 the terms become:
• For the first term, v^(5/2) = v^(7/2–1) so s = 7/2:
  I₁ = Γ(7/2)·4^(7/2).
• For the second term, v^(3/2) = v^(5/2–1) so s = 5/2:
  I₂ = Γ(5/2)·4^(5/2).
• For the third term, v^(1/2) = v^(3/2–1) so s = 3/2:
  I₃ = Γ(3/2)·4^(3/2).

Thus,
  I = (e^(–1/4)/(2)) [ Γ(7/2)·4^(7/2) – 10 Γ(5/2)·4^(5/2) + Γ(3/2)·4^(3/2) ].

Step 4. Substitute the known Gamma values and simplify.

We have:
  Γ(3/2) = (√π)/2,
  Γ(5/2) = (3√π)/4,
  Γ(7/2) = (15√π)/8.
Also note that 4^(n/2) = 2^n. Hence:
  4^(7/2) = 2⁷ = 128,
  4^(5/2) = 2⁵ = 32,
  4^(3/2) = 2³ = 8.

Now substitute these:
  I = (e^(–1/4)/(2)) [ (15√π/8)*128 – 10*(3√π/4)*32 + (√π/2)*8 ].
Simplify each term:
• First term: (15√π/8)*128 = 15√π·16 = 240√π.
• Second term: 10*(3√π/4)*32 = 10·3√π·8 = 240√π.
• Third term: (√π/2)*8 = 4√π.

Thus the bracket becomes:
  240√π – 240√π + 4√π = 4√π.
Then,
  I = (e^(–1/4)/(2))·4√π = 2√π e^(–1/4).

Step 5. Numerical approximation.

We have:
  √π ≈ 1.7724538509,
so
  2√π ≈ 3.5449077018.
Also, e^(–1/4) = e^(–0.25) ≈ 0.7788007831.
Thus,
  I ≈ 3.5449077018 × 0.7788007831 ≈ 2.7621742633.

Final Answer in JSON:
{"answer": "2\\sqrt{\\pi}e^{-\\frac{1}{4}}", "numerical_answer": "2.7621742633"}