We wish to evaluate

  I = ∫₁² (9x + 4)/(x⁵ + 3x² + x) dx.

Step 1. Factor the denominator.
Notice that
  x⁵ + 3x² + x = x (x⁴ + 3x + 1).

Thus, the integrand becomes
  (9x + 4)/[x (x⁴ + 3x + 1)].

Step 2. Express the integrand as a derivative.
We look for constants a and b such that

  d/dx ln[(x⁴ + 3x + 1)ᵃ · xᵇ] = (9x + 4)/[x (x⁴ + 3x + 1)].

Using the chain rule, we have

  d/dx ln[(x⁴ + 3x + 1)ᵃ xᵇ] = (a (4x³ + 3))/(x⁴ + 3x + 1) + b/x.
  Combine these into one fraction:
  = [a (4x³ + 3)x + b (x⁴ + 3x + 1)]/[x (x⁴ + 3x + 1)].

Expand the numerator:
  = [(4a + b)x⁴ + (3a + 3b)x + b] / [x (x⁴ + 3x + 1)].

This expression must equal (9x + 4)/[x (x⁴ + 3x + 1)]. Hence we equate coefficients:
  Coefficient of x⁴: 4a + b = 0.      (1)
  Coefficient of x: 3a + 3b = 9.     (2)
  Constant term: b = 4.        (3)

From (3) we have b = 4. Substitute into (1):
  4a + 4 = 0  ⟹  a = -1.
Now check (2):
  3(–1) + 3(4) = –3 + 12 = 9.
This is consistent.

Thus, we have
  d/dx ln[(x⁴ + 3x + 1)^(–1) · x⁴] = (9x + 4)/[x (x⁴ + 3x + 1)].

That is, the antiderivative is
  F(x) = ln( x⁴/(x⁴ + 3x + 1) ).

Step 3. Evaluate the integral.
Now compute F(2) and F(1).

For x = 2:
  x⁴ = 2⁴ = 16,
  x⁴ + 3x + 1 = 16 + 6 + 1 = 23,
  So, F(2) = ln(16/23).

For x = 1:
  x⁴ = 1,
  x⁴ + 3x + 1 = 1 + 3 + 1 = 5,
  So, F(1) = ln(1/5).

Thus, the value of the definite integral is
  I = F(2) – F(1) = ln(16/23) – ln(1/5) = ln( (16/23) · 5 ) = ln(80/23).

Step 4. Provide a numerical approximation.
We have
  I = ln(80/23).
Computing the value:
  80/23 ≈ 3.4782608695652174,
  ln(3.4782608695652174) ≈ 1.2465324177.

Final Answer in JSON:
{"answer": "\\ln\\left(\\frac{80}{23}\\right)", "numerical_answer": "1.2465324177"}