<think>
Okay, so I need to compute the definite integral from 0 to 1 of x times arcsin x times arccos x dx. Hmm, let's start by understanding the problem. The integrand is x multiplied by both arcsin x and arccos x. I remember that arcsin and arccos are related; specifically, arcsin x + arccos x equals π/2. Maybe that identity can help simplify things here. Let me write that down: arcsin x + arccos x = π/2. 

So, perhaps, I can express one of the inverse trigonometric functions in terms of the other. Let's say, replace arccos x with π/2 - arcsin x. Then the product arcsin x * arccos x becomes arcsin x * (π/2 - arcsin x). That might make the integral more manageable. Let me try substituting that in.

So the integrand becomes x * arcsin x * (π/2 - arcsin x). Expanding that, it's x*(π/2 arcsin x - (arcsin x)^2). Therefore, the integral splits into two parts: (π/2) times the integral of x arcsin x dx minus the integral of x (arcsin x)^2 dx. 

Let me write that as:

Integral = (π/2) ∫₀¹ x arcsin x dx - ∫₀¹ x (arcsin x)^2 dx

Now, I need to compute these two integrals separately. Let's start with the first one: ∫ x arcsin x dx. For this, integration by parts might be useful. Let me recall that integration by parts formula: ∫u dv = uv - ∫v du. 

Let me set u = arcsin x, which means du = 1/√(1 - x²) dx. Then dv = x dx, so v = (1/2)x². Applying integration by parts:

∫ x arcsin x dx = (1/2)x² arcsin x - ∫ (1/2)x² * (1/√(1 - x²)) dx

Simplify the remaining integral: (1/2) ∫ x² / √(1 - x²) dx. Hmm, this integral might require a substitution. Let me set t = 1 - x², so dt = -2x dx. Wait, but the integral has x² over √(1 - x²). Maybe another substitution. Alternatively, express x² as (1 - (1 - x²)) so:

x² / √(1 - x²) = [1 - (1 - x²)] / √(1 - x²) = 1/√(1 - x²) - √(1 - x²)

Therefore, the integral becomes (1/2) [∫1/√(1 - x²) dx - ∫√(1 - x²) dx]

Compute these integrals:

∫1/√(1 - x²) dx is arcsin x + C

∫√(1 - x²) dx is a standard integral. Let me recall that ∫√(a² - x²) dx = (x/2)√(a² - x²) + (a²/2) arcsin(x/a) + C. Here, a=1, so it becomes (x/2)√(1 - x²) + (1/2) arcsin x + C

Putting it all together:

(1/2)[arcsin x - (x/2)√(1 - x²) - (1/2) arcsin x] + C

Simplify:

(1/2)[ (arcsin x - (1/2) arcsin x ) - (x/2)√(1 - x²) ]

Which is (1/2)[ (1/2) arcsin x - (x/2)√(1 - x²) ] + C

So, (1/4) arcsin x - (x/4)√(1 - x²) + C

Therefore, going back to the first integral:

∫ x arcsin x dx = (1/2)x² arcsin x - [ (1/4) arcsin x - (x/4)√(1 - x²) ] + C

Wait, but we need to evaluate the definite integral from 0 to 1. Let's compute the definite integral:

From 0 to 1:

First term: (1/2)(1)^2 arcsin(1) - (1/4) arcsin(1) + (1/4)(1)√(1 - 1^2) 

Minus the same expression evaluated at 0:

(1/2)(0)^2 arcsin(0) - (1/4) arcsin(0) + (0/4)√(1 - 0^2)

Compute each part:

At x=1:

arcsin(1) = π/2, √(1 - 1) = 0

So first term at 1: (1/2)(π/2) - (1/4)(π/2) + 0 = (π/4) - (π/8) = π/8

At x=0:

arcsin(0) = 0, so all terms are 0.

Therefore, the first integral ∫₀¹ x arcsin x dx = π/8

So the first part of our original integral is (π/2)*(π/8) = π²/16

Now, moving on to the second integral: ∫₀¹ x (arcsin x)^2 dx

This seems more complicated. Let's tackle this integral. Again, integration by parts might be needed. Let me set u = (arcsin x)^2, dv = x dx

Then du = 2 arcsin x * (1/√(1 - x²)) dx, and v = (1/2)x²

So, integration by parts gives:

∫ x (arcsin x)^2 dx = (1/2)x² (arcsin x)^2 - ∫ (1/2)x² * 2 arcsin x / √(1 - x²) dx

Simplify: (1/2)x² (arcsin x)^2 - ∫ x² arcsin x / √(1 - x²) dx

Hmm, the remaining integral is ∫ x² arcsin x / √(1 - x²) dx. Let's see if we can handle this. Let me make a substitution here. Let t = arcsin x. Then x = sin t, dx = cos t dt. Also, √(1 - x²) = cos t. So substituting:

x = sin t, so x² = sin² t, arcsin x = t, and √(1 - x²) = cos t. Therefore, the integral becomes:

∫ (sin² t) * t / cos t) * cos t dt = ∫ t sin² t dt

Because the cos t cancels with the denominator. So the integral simplifies to ∫ t sin² t dt. Let's compute that.

First, let's recall that sin² t = (1 - cos 2t)/2. So:

∫ t sin² t dt = ∫ t*(1 - cos 2t)/2 dt = (1/2) ∫ t dt - (1/2) ∫ t cos 2t dt

Compute each integral:

First integral: (1/2)*(t²/2) = t²/4

Second integral: (1/2) ∫ t cos 2t dt. Use integration by parts here. Let u = t, dv = cos 2t dt. Then du = dt, v = (1/2) sin 2t

So, ∫ t cos 2t dt = t*(1/2) sin 2t - ∫ (1/2) sin 2t dt = (t/2) sin 2t + (1/4) cos 2t + C

Therefore, the second integral becomes (1/2)[ (t/2) sin 2t + (1/4) cos 2t ] + C

Putting it all together:

∫ t sin² t dt = t²/4 - (1/2)[ (t/2) sin 2t + (1/4) cos 2t ] + C

Simplify:

= t²/4 - (t/4) sin 2t - (1/8) cos 2t + C

Now, revert back to x. Remember t = arcsin x. So:

= (arcsin x)^2 /4 - (arcsin x)/4 * sin(2 arcsin x) - (1/8) cos(2 arcsin x) + C

Simplify the trigonometric terms. Let's compute sin(2 arcsin x) and cos(2 arcsin x).

First, sin(2θ) = 2 sinθ cosθ. Here θ = arcsin x, so sinθ = x, cosθ = √(1 - x²). Therefore, sin(2 arcsin x) = 2x√(1 - x²)

For cos(2θ), we can use cos(2θ) = 1 - 2 sin²θ = 1 - 2x²

Therefore, substituting back:

= (arcsin x)^2 /4 - (arcsin x)/4 * 2x√(1 - x²) - (1/8)(1 - 2x²) + C

Simplify:

= (arcsin x)^2 /4 - (arcsin x x √(1 - x²))/2 - (1/8) + (x²)/4 + C

Therefore, the integral ∫ x (arcsin x)^2 dx is:

(1/2)x² (arcsin x)^2 - [ (arcsin x)^2 /4 - (arcsin x x √(1 - x²))/2 - 1/8 + x²/4 ] + C

Wait, let's check. The original integral after integration by parts was:

(1/2)x² (arcsin x)^2 - ∫ x² arcsin x / √(1 - x²) dx

And we found that ∫ x² arcsin x / √(1 - x²) dx = (arcsin x)^2 /4 - (arcsin x x √(1 - x²))/2 - 1/8 + x²/4 + C

Therefore, the integral becomes:

(1/2)x² (arcsin x)^2 - [ (arcsin x)^2 /4 - (arcsin x x √(1 - x²))/2 - 1/8 + x²/4 ] + C

Simplify the expression:

= (1/2)x² (arcsin x)^2 - (arcsin x)^2 /4 + (arcsin x x √(1 - x²))/2 + 1/8 - x²/4 + C

Now, we need to evaluate this definite integral from 0 to 1.

Let's compute each term at the limits 1 and 0.

First, at x=1:

arcsin(1) = π/2, √(1 - 1) = 0, x=1.

So:

Term1: (1/2)(1)^2 (π/2)^2 = (1/2)(π²/4) = π²/8

Term2: - (π/2)^2 /4 = - π²/(16)

Term3: (π/2 * 1 * 0)/2 = 0

Term4: +1/8

Term5: - (1)^2 /4 = -1/4

So total at x=1: π²/8 - π²/16 + 0 + 1/8 - 1/4

Simplify:

π²/8 - π²/16 = π²/16

1/8 - 1/4 = -1/8

So total: π²/16 - 1/8

Now, at x=0:

arcsin(0) = 0, x=0.

Term1: (1/2)(0)^2 (0)^2 = 0

Term2: - (0)^2 /4 = 0

Term3: (0 * 0 * 1)/2 = 0

Term4: +1/8

Term5: -0^2 /4 = 0

So total at x=0: 0 - 0 + 0 + 1/8 - 0 = 1/8

Therefore, the definite integral from 0 to 1 is [π²/16 - 1/8] - [1/8] = π²/16 - 1/8 - 1/8 = π²/16 - 1/4

So ∫₀¹ x (arcsin x)^2 dx = π²/16 - 1/4

Putting it all back into the original integral:

Original Integral = (π/2)(π/8) - (π²/16 - 1/4) = π²/16 - π²/16 + 1/4 = 1/4

Wait, that's interesting. Let me check that again.

Original Integral = (π/2)*∫x arcsin x dx - ∫x (arcsin x)^2 dx

We found ∫x arcsin x dx = π/8, so (π/2)*(π/8) = π²/16

Then subtract ∫x (arcsin x)^2 dx = π²/16 - 1/4

So π²/16 - (π²/16 - 1/4) = π²/16 - π²/16 + 1/4 = 1/4

So the result is 1/4? That seems surprisingly simple. Let me verify this.

Wait, maybe I made a mistake in the calculation. Let me check the steps again.

First, the first integral was ∫₀¹ x arcsin x dx = π/8. Then, the second integral was ∫₀¹ x (arcsin x)^2 dx = π²/16 - 1/4. Then, the original integral is (π/2)(π/8) - (π²/16 - 1/4) = π²/16 - π²/16 + 1/4 = 1/4. So yes, the result is 1/4. That seems correct. Let me check with a numerical approximation to see if it's plausible.

But 1/4 is 0.25. Let me compute the integral numerically to check. Let's take x from 0 to 1, and compute x*arcsin(x)*arccos(x). Let's approximate it numerically. For example, at x=0.5, arcsin(0.5)=π/6≈0.5236, arccos(0.5)=π/3≈1.0472, so product is 0.5*0.5236*1.0472≈0.5*0.548≈0.274. So the integrand is positive in the interval, and the integral from 0 to 1 would be some positive value. 0.25 is plausible. Let me check with x=1: arcsin(1)=π/2≈1.5708, arccos(1)=0, so the integrand is 0. At x=0, similar. The function starts at 0, goes up, and comes back to 0. The integral being 0.25 seems possible. Let me compute a rough numerical approximation.

Alternatively, since the exact answer is 1/4, which is 0.25, the numerical approximation should be 0.25. Let me check with a simple method. Let's use substitution. Let x = sinθ, then dx = cosθ dθ. When x=0, θ=0; x=1, θ=π/2. Then the integral becomes ∫₀^{π/2} sinθ * θ * (π/2 - θ) * cosθ dθ. That's ∫₀^{π/2} θ(π/2 - θ) sinθ cosθ dθ. Let me make substitution u = θ, v = π/2 - θ. But maybe expand the product: θ(π/2 - θ) = (π/2)θ - θ². So the integral is ∫₀^{π/2} [(π/2)θ - θ³] sinθ cosθ dθ. Wait, sinθ cosθ is (1/2) sin2θ. So the integral becomes (1/2) ∫₀^{π/2} [ (π/2)θ - θ³ ] sin2θ dθ. Let me split this into two integrals:

(π/4) ∫₀^{π/2} θ sin2θ dθ ) - (1/2) ∫₀^{π/2} θ³ sin2θ dθ

Compute these integrals. Let's compute the first one: ∫θ sin2θ dθ. Integration by parts. Let u = θ, dv = sin2θ dθ. Then du = dθ, v = - (1/2) cos2θ. So ∫θ sin2θ dθ = - (θ/2) cos2θ + (1/2) ∫cos2θ dθ = - (θ/2) cos2θ + (1/4) sin2θ. Evaluated from 0 to π/2:

At π/2: - (π/4) cosπ + (1/4) sinπ = - (π/4)(-1) + 0 = π/4

At 0: -0 + 0 = 0

So first integral is π/4. Multiply by π/4: (π/4)*(π/4) = π²/16

Now the second integral: ∫θ³ sin2θ dθ. This will require multiple integration by parts. Let me set u = θ³, dv = sin2θ dθ. Then du = 3θ² dθ, v = - (1/2) cos2θ

First step: - (θ³/2) cos2θ + (3/2) ∫θ² cos2θ dθ

Now, compute ∫θ² cos2θ dθ. Again, integration by parts. Let u = θ², dv = cos2θ dθ. Then du = 2θ dθ, v = (1/2) sin2θ

So ∫θ² cos2θ dθ = (θ²/2) sin2θ - ∫θ sin2θ dθ

We already know ∫θ sin2θ dθ from before, which was π/4 when evaluated from 0 to π/2. Wait, but here it's indefinite. Wait, but in this case, we need to compute ∫θ sin2θ dθ as part of the process. Let's proceed.

So ∫θ² cos2θ dθ = (θ²/2) sin2θ - [ - (θ/2) cos2θ + (1/4) sin2θ ] + C

= (θ²/2) sin2θ + (θ/2) cos2θ - (1/4) sin2θ + C

Therefore, going back to the previous step:

- (θ³/2) cos2θ + (3/2)[ (θ²/2) sin2θ + (θ/2) cos2θ - (1/4) sin2θ ] evaluated from 0 to π/2

Let's evaluate each term at π/2 and 0.

At θ=π/2:

First term: - ( (π/2)^3 /2 ) cosπ = - (π³/16)(-1) = π³/16

Second term: (3/2)[ ( (π/2)^2 /2 ) sinπ + (π/4) cosπ - (1/4) sinπ ]

= (3/2)[ 0 + (π/4)(-1) - 0 ] = (3/2)( -π/4 ) = -3π/8

Third term: (3/2)[ - (1/4) sinπ ] = 0

At θ=0:

All terms are 0 because sin0=0 and cos0=1 multiplied by 0.

So total for the second integral:

[ π³/16 - 3π/8 ] - 0 = π³/16 - 3π/8

Therefore, the second integral is:

- (1/2) [ π³/16 - 3π/8 ] = - π³/32 + 3π/16

Putting it all together, the original integral via substitution is:

π²/16 - ( - π³/32 + 3π/16 ) = π²/16 + π³/32 - 3π/16

Wait, this contradicts the previous result of 1/4. Hmm, this suggests a mistake. But earlier steps gave 1/4, but this substitution method is leading to a different result. There must be an error in one of the methods.

Wait, no. Wait, the substitution method was an alternative approach. Let me check again. Wait, the substitution method was supposed to compute the same integral, but I might have messed up the steps. Let me recap:

Original integral via substitution became:

(π/4)*(π/4) - (1/2)*(π³/16 - 3π/8) = π²/16 - (π³/32 - 3π/16)

= π²/16 - π³/32 + 3π/16

But this is different from the previous result of 1/4. Therefore, there must be a mistake in one of the methods. Let's check the first method again.

In the first method, after computing both integrals, we found the result to be 1/4. But in the substitution method, it's giving a different answer. Therefore, one of the methods must have an error.

Wait, but the substitution method is more complicated, so perhaps I made a mistake there. Let me check the substitution steps again.

Wait, when I did the substitution x = sinθ, then the integral becomes ∫θ(π/2 - θ) sinθ cosθ dθ from 0 to π/2. Then, expanding that gives (π/2)θ - θ², multiplied by sinθ cosθ. Then, sinθ cosθ is (1/2) sin2θ. So the integral becomes (1/2) ∫ [ (π/2)θ - θ² ] sin2θ dθ. Then, split into two parts: (π/4) ∫θ sin2θ dθ - (1/2) ∫θ² sin2θ dθ. Wait, no, the second term is ∫θ² sin2θ dθ? Wait, no, expanding [ (π/2)θ - θ² ] * sin2θ/2, so the integral is (π/4) ∫θ sin2θ dθ - (1/2) ∫θ² sin2θ dθ. Wait, but in the substitution method, I think I made a mistake in splitting the terms. Let me re-express:

Original substitution integral:

∫₀¹ x arcsin x arccos x dx = ∫₀^{π/2} sinθ * θ * (π/2 - θ) * cosθ dθ

= ∫₀^{π/2} θ(π/2 - θ) sinθ cosθ dθ

= ∫₀^{π/2} [ (π/2)θ - θ² ] sinθ cosθ dθ

Now, sinθ cosθ = (1/2) sin2θ, so:

= (1/2) ∫₀^{π/2} [ (π/2)θ - θ² ] sin2θ dθ

= (π/4) ∫₀^{π/2} θ sin2θ dθ - (1/2) ∫₀^{π/2} θ² sin2θ dθ

Yes, that's correct. Then, compute each integral.

First integral: ∫θ sin2θ dθ from 0 to π/2. As before, this is π/4.

Second integral: ∫θ² sin2θ dθ from 0 to π/2. Let's compute this again.

Let me use integration by parts. Let u = θ², dv = sin2θ dθ. Then du = 2θ dθ, v = - (1/2) cos2θ

So ∫θ² sin2θ dθ = - (θ²/2) cos2θ + ∫θ cos2θ dθ

Now, compute ∫θ cos2θ dθ. Again, integration by parts. Let u = θ, dv = cos2θ dθ. Then du = dθ, v = (1/2) sin2θ

So ∫θ cos2θ dθ = (θ/2) sin2θ - (1/2) ∫ sin2θ dθ = (θ/2) sin2θ + (1/4) cos2θ + C

Therefore, the integral becomes:

- (θ²/2) cos2θ + (θ/2) sin2θ + (1/4) cos2θ evaluated from 0 to π/2

At θ=π/2:

- ( (π/2)^2 /2 ) cosπ + (π/4) sinπ + (1/4) cosπ

= - (π²/8)(-1) + 0 + (1/4)(-1) = π²/8 - 1/4

At θ=0:

-0 + 0 + (1/4)(1) = 1/4

So the definite integral is (π²/8 - 1/4) - (1/4) = π²/8 - 1/2

Therefore, the second integral ∫θ² sin2θ dθ from 0 to π/2 is π²/8 - 1/2

Therefore, going back to the substitution integral:

= (π/4)(π/4) - (1/2)(π²/8 - 1/2)

= π²/16 - (π²/16 - 1/4)

= π²/16 - π²/16 + 1/4

= 1/4

Ah! So this matches the previous result. So the substitution method also gives 1/4. Therefore, the original integral is indeed 1/4. So the first method was correct. I must have made a mistake in the substitution method when I first tried to compute the second integral. But upon re-evaluating, it also gives 1/4. Therefore, the exact answer is 1/4, which is 0.25. Therefore, the numerical approximation is 0.25, which is already exact to 10 decimal places. So the numerical approximation is 0.2500000000.

Therefore, the final answer is 1/4, and the numerical approximation is 0.25.
</think>

{"answer": "\\frac{1}{4}", "numerical_answer": 0.2500000000}