Let's solve the integral:
\[
I = \int_0^\infty \frac{1}{e^x+1}\,dx
\]

### Step 1: Analytical Solution

We'll begin by finding a way to express the integrand in a form that allows us to integrate it.

#### Expressing as a Series

Note that:
\[
\frac{1}{e^x+1} = \sum_{n=1}^\infty (-1)^{n+1} e^{-nx}
\]
This series converges for all \(x > 0\) (this is a standard geometric series manipulation).

**Proof:**  
Recall the geometric series:
\[
\frac{1}{1 + y} = \sum_{n=1}^\infty (-1)^{n+1} y^{n-1}, \quad |y| < 1
\]
Set \(y = e^{-x}\) (where \(0 < y < 1\) for \(x > 0\)):
\[
\frac{1}{1+e^{-x}} = \sum_{n=1}^\infty (-1)^{n+1} e^{-x(n-1)}
\]
\[
\frac{1}{e^{x}+1} = \frac{e^{-x}}{1+e^{-x}} = \sum_{n=1}^\infty (-1)^{n+1} e^{-nx}
\]

#### Integrate Term by Term

Therefore,
\[
I = \int_0^\infty \sum_{n=1}^\infty (-1)^{n+1} e^{-nx} dx = \sum_{n=1}^\infty (-1)^{n+1} \int_0^\infty e^{-nx} dx
\]
\[
\int_0^\infty e^{-nx} dx = \left[ -\frac{1}{n} e^{-nx} \right]_0^\infty = 0 - \left(-\frac{1}{n}\right) = \frac{1}{n}
\]
So,
\[
I = \sum_{n=1}^\infty \frac{(-1)^{n+1}}{n}
\]
This is the alternating harmonic series, whose sum is \(\ln 2\):

\[
\sum_{n=1}^\infty \frac{(-1)^{n+1}}{n} = \ln 2
\]

### Step 2: Exact Analytical Answer

\[
\boxed{I = \ln 2}
\]

### Step 3: Numerical Approximation

\[
\ln 2 \approx 0.6931471806
\]

### Step 4: JSON Output

```json
{"answer": "\\ln 2", "numerical_answer": "0.6931471806"}
```