
To solve the definite integral \(\int_0^1 \frac{\sin(\log x) - \log x}{\log^2 x} \, dx\), we proceed with the following steps:

### Step 1: Substitution
Let \( t = \log x \). Then \( x = e^t \), \( dx = e^t dt \). When \( x = 0 \), \( t \to -\infty \); when \( x = 1 \), \( t = 0 \). The integral transforms to:
\[
\int_{-\infty}^0 \frac{\sin(t) - t}{t^2} e^t \, dt
\]

### Step 2: Change of Variable
Let \( s = -t \), so \( t = -s \), \( dt = -ds \). The limits change from \( t \to -\infty \) ( \( s \to \infty \)) to \( t = 0 \) ( \( s = 0 \)). The integral becomes:
\[
\int_{\infty}^0 \frac{\sin(-s) - (-s)}{(-s)^2} e^{-s} (-ds) = \int_0^\infty \frac{s - \sin s}{s^2} e^{-s} \, ds
\]

### Step 3: Integrate by Parts
Consider \( I = \int_0^\infty \frac{s - \sin s}{s^2} e^{-s} \, ds \). Let \( u = (s - \sin s)e^{-s} \) and \( dv = \frac{ds}{s^2} \). Then \( du = e^{-s}(1 - \cos s - s + \sin s) \, ds \) and \( v = -\frac{1}{s} \). Integration by parts gives:
\[
I = \left[ -\frac{(s - \sin s)e^{-s}}{s} \right]_0^\infty + \int_0^\infty \frac{e^{-s}(1 - \cos s - s + \sin s)}{s} \, ds
\]
The boundary terms vanish (verified by limits as \( s \to 0 \) and \( s \to \infty \)). Thus:
\[
I = \int_0^\infty e^{-s} \left( \frac{1 - s}{s} + \frac{\sin s - \cos s}{s} \right) ds
\]

### Step 4: Evaluate Integrals
Split \( I \) into two parts:
\[
I = \int_0^\infty e^{-s} \frac{1 - s}{s} \, ds + \int_0^\infty e^{-s} \frac{\sin s - \cos s}{s} \, ds
\]

- **First Integral**: \( \int_0^\infty e^{-s} \frac{1 - s}{s} \, ds = \int_0^\infty \left( \frac{e^{-s}}{s} - e^{-s} \right) ds \). This simplifies using properties of exponential integrals, but combined with the second integral, divergences cancel.
- **Second Integral**: Use Laplace transforms and known integrals. For \( \int_0^\infty e^{-s} \frac{\sin s}{s} \, ds = \frac{\pi}{4} \) and \( \int_0^\infty e^{-s} \frac{\cos s}{s} \, ds = \frac{1}{2} \ln 2 \). Thus:
\[
\int_0^\infty e^{-s} \frac{\sin s - \cos s}{s} \, ds = \frac{\pi}{4} + \frac{1}{2} \ln 2
\]

### Step 5: Combine Results
Combining these, the integral simplifies to:
\[
I = -1 + \frac{\pi}{4} + \frac{1}{2} \ln 2
\]

### Numerical Approximation
Using \( \pi \approx 3.1415926536 \) and \( \ln 2 \approx 0.6931471806 \):
\[
I \approx -1 + \frac{3.1415926536}{4} + \frac{0.6931471806}{2} \approx 0.1319717537
\]

### Final Answer
{"answer": "\(-1 + \frac{\pi}{4} + \frac{1}{2} \ln 2\)", "numerical_answer": "0.1319717537"}