We wish to evaluate

  I = ∫₁³ [ln(x)/(x² + 3)] dx.

A very clever change of variable makes the answer apparent. We first substitute

  t = x/√3   ⟹   x = √3·t   and  dx = √3 dt.

The limits change as follows:
  when x = 1, t = 1/√3,  
  when x = 3, t = 3/√3 = √3.

Then the denominator becomes
  x² + 3 = 3t² + 3 = 3(t² + 1).

Thus the integral becomes

  I = ∫₁³ [ln(x)/(x² + 3)] dx
    = ∫₁/√3^(√3) [ln(√3·t)/(3(t² + 1))] (√3 dt)
    = (√3/3) ∫₁/√3^(√3) [ln(√3·t)/(t² + 1)] dt.

Now write
  ln(√3·t) = ln(t) + ln(√3).

Thus we split the integral into two pieces:

  I = (√3/3) { ∫₁/√3^(√3) [ln(t)/(t² + 1)] dt + ln(√3) ∫₁/√3^(√3) [1/(t² + 1)] dt }.

Observe that the integration interval for t is from 1/√3 to √3 and note that these endpoints are reciprocals:
  (1/√3) × (√3) = 1.

• First, consider
  A = ∫₁/√3^(√3) [ln(t)/(t² + 1)] dt.
Make the substitution u = 1/t. Then du = –dt/t² and (t²+1) is symmetric under t ↔ 1/t. One may show that under this substitution A changes sign. Since the limits swap (because 1/(1/√3)=√3 and 1/(√3)=1/√3), one finds that A = –A and hence
  A = 0.

• Next, the second integral is
  B = ∫₁/√3^(√3) [1/(t² + 1)] dt = [arctan(t)]₁/√3^(√3) = arctan(√3) – arctan(1/√3).
But
  arctan(√3) = π/3  and  arctan(1/√3) = π/6,
so
  B = (π/3 – π/6) = π/6.

Thus, our integral reduces to

  I = (√3/3)[0 + ln(√3) · (π/6)]
    = (√3 π ln(√3))/(18).

Since ln(√3) = (1/2) ln 3, we can write

  I = (√3 π (ln 3)/2)/(18) = (π √3 ln 3)/36.

This is the exact answer.

To obtain a numerical approximation, we compute:
  π ≈ 3.1415926536,
  √3 ≈ 1.7320508076,
  ln 3 ≈ 1.0986122887.
Then:
  π √3 ln 3 ≈ 3.1415926536 × 1.7320508076 × 1.0986122887 ≈ 5.984493142,
so
  I ≈ 5.984493142/36 ≈ 0.1662369217.

Rounded to 10 decimal places the numerical answer is 0.1662369217.

The final result in the required JSON format is:
{"answer": "$\\frac{\\pi\\sqrt{3}\\ln 3}{36}$", "numerical_answer": "0.1662369217"}