# Evaluating $\int\limits_0^2x^{-1/2}H_{3}\left(\sqrt[4]{x(2-x)}\right)dx$

First, I need to identify what $H_3(x)$ represents. This is the Hermite polynomial of degree 3, which is:
$H_3(x) = 8x^3 - 12x$

## Step 1: Substitute the Hermite polynomial
Let's substitute $u = \sqrt[4]{x(2-x)}$, so:
$$\int\limits_0^2x^{-1/2}H_{3}\left(\sqrt[4]{x(2-x)}\right)dx = \int\limits_0^2x^{-1/2}(8(\sqrt[4]{x(2-x)})^3 - 12\sqrt[4]{x(2-x)})dx$$
$$= \int\limits_0^2x^{-1/2}(8(x(2-x))^{3/4} - 12(x(2-x))^{1/4})dx$$

## Step 2: Use symmetry of the interval
I notice that this integral is over $[0,2]$. Let's make a substitution $x = 2-y$, which maps $x=0$ to $y=2$ and $x=2$ to $y=0$.

Under this substitution:
- $dx = -dy$
- $x^{-1/2} = (2-y)^{-1/2}$
- $x(2-x) = (2-y)y$

So the integral becomes:
$$\int\limits_0^2(2-y)^{-1/2}(8((2-y)y)^{3/4} - 12((2-y)y)^{1/4})(-dy)$$
$$= -\int\limits_2^0(2-y)^{-1/2}(8((2-y)y)^{3/4} - 12((2-y)y)^{1/4})dy$$
$$= \int\limits_0^2(2-y)^{-1/2}(8((2-y)y)^{3/4} - 12((2-y)y)^{1/4})dy$$

Note that $(2-y)y = y(2-y)$, so the expressions inside the Hermite polynomial remain the same.

## Step 3: Add the original and transformed integrals
Adding our original integral and the transformed version:

$$2\int\limits_0^2x^{-1/2}H_{3}\left(\sqrt[4]{x(2-x)}\right)dx = \int\limits_0^2(x^{-1/2} + (2-x)^{-1/2})H_{3}\left(\sqrt[4]{x(2-x)}\right)dx$$

## Step 4: Observe the symmetry of the integrand
Since the term $x(2-x)$ is symmetric around $x=1$, and $H_3$ is an odd function for odd indices (meaning $H_3(-x) = -H_3(x)$), we need to carefully analyze how this affects our integral.

Let's use the property that:
$x^{-1/2} + (2-x)^{-1/2} = \frac{1}{\sqrt{x}} + \frac{1}{\sqrt{2-x}}$

This expression is symmetric around $x=1$ because if we substitute $x' = 2-x$, we get $\frac{1}{\sqrt{2-x'}} + \frac{1}{\sqrt{x'}}$.

## Step 5: Evaluate the integral
Due to the symmetry properties, and since $H_3$ is an odd function applied to an even function of $x$ around $x=1$, the integral evaluates to 0.

Therefore:
$$\int\limits_0^2x^{-1/2}H_{3}\left(\sqrt[4]{x(2-x)}\right)dx = 0$$

## Numerical Approximation
The exact answer is 0, so the numerical approximation rounded to 10 decimal places is also 0.0000000000.

{"answer": "0", "numerical_answer": "0.0000000000"}