We wish to evaluate

  I = ∫ from -1 to 1 (5x³ – 3x)² dx.

Step 1. Expand the integrand.

  (5x³ – 3x)² = (5x³)² – 2·5x³·3x + (3x)²
       = 25x⁶ – 30x⁴ + 9x².

Step 2. Write the integral in terms of the expanded polynomial.

  I = ∫ from -1 to 1 (25x⁶ – 30x⁴ + 9x²) dx.

Step 3. Notice that each term (x⁶, x⁴, x²) is an even function. When integrating an even function over the symmetric interval [-a, a] the integral is twice the integral from 0 to a. Alternatively, we can directly integrate knowing that

  ∫ from -1 to 1 xⁿ dx = 2/(n + 1) (if n is even).

Compute each term:
  ∫_(-1)^(1) 25x⁶ dx = 25 · (2/7) = 50/7
  ∫_(-1)^(1) (-30x⁴) dx = -30 · (2/5) = -12
  ∫_(-1)^(1) 9x² dx = 9 · (2/3) = 6

Step 4. Sum the results.

  I = (50/7) – 12 + 6 = 50/7 – 6.
    Express 6 as 42/7:
    I = (50 – 42)/7 = 8/7.

Step 5. Provide the numerical approximation.

  8/7 ≈ 1.142857142857... 
  Rounded to 10 decimal places: 1.1428571429.

Thus the final answer is:

{"answer": "\frac{8}{7}", "numerical_answer": "1.1428571429"}