To evaluate the definite integral

$$
\int_0^{2} x^{-1/2} \left[1 + \sqrt{x(2 - x)}\right]^{-3/2} dx,
$$

we begin by recognizing the structure of the integrand. The expression inside the square root, $ x(2 - x) $, can be rewritten as:

$$
x(2 - x) = 1 - (x - 1)^2,
$$

which suggests a trigonometric substitution due to the form $ 1 - \theta^2 $, reminiscent of the identity $ \sin^2\theta + \cos^2\theta = 1 $.

---

### Step 1: Substitution

Letâ€™s perform the substitution:

$$
x = 1 + \sin\phi \quad \Rightarrow \quad dx = \cos\phi \, d\phi.
$$

When $ x = 0 $, $ \phi = -\frac{\pi}{2} $, and when $ x = 2 $, $ \phi = \frac{\pi}{2} $.

Now rewrite the integral in terms of $ \phi $:

$$
\int_0^2 x^{-1/2} \left[1 + \sqrt{x(2 - x)}\right]^{-3/2} dx = \int_{-\frac{\pi}{2}}^{\frac{\pi}{2}} (1 + \sin\phi)^{-1/2} \left[1 + \cos\phi\right]^{-3/2} \cos\phi \, d\phi.
$$

---

### Step 2: Simplify Using Trigonometric Identities

We use the identities:

- $ 1 + \sin\phi = 2\sin^2\left(\frac{\phi}{2} + \frac{\pi}{4}\right) $, so $ (1 + \sin\phi)^{-1/2} = \frac{1}{\sqrt{2} \sin\left(\frac{\phi}{2} + \frac{\pi}{4}\right)} $,
- $ 1 + \cos\phi = 2\cos^2\left(\frac{\phi}{2}\right) $, so $ (1 + \cos\phi)^{-3/2} = \frac{1}{2^{3/2} \cos^3\left(\frac{\phi}{2}\right)} $,
- $ \cos\phi = \cos\left(\frac{\phi}{2} + \frac{\phi}{2}\right) = \cos^2\left(\frac{\phi}{2}\right) - \sin^2\left(\frac{\phi}{2}\right) $.

After simplifying the integrand and factoring constants, we arrive at:

$$
\int_{-\frac{\pi}{2}}^{\frac{\pi}{2}} \frac{\cos\phi}{(1 + \sin\phi)^{1/2}(1 + \cos\phi)^{3/2}} d\phi = \int_{-\frac{\pi}{2}}^{\frac{\pi}{2}} \frac{1}{2^{3/2}} \cdot \frac{\cos\phi}{\sin\left(\frac{\phi}{2} + \frac{\pi}{4}\right) \cdot \cos^3\left(\frac{\phi}{2}\right)} d\phi.
$$

This can be further simplified using substitution:

Let $ u = \tan\left(\frac{\phi}{2}\right) $, so $ du = \frac{1}{2} \sec^2\left(\frac{\phi}{2}\right) d\phi $, and $ \sec^2\left(\frac{\phi}{2}\right) d\phi = 2 du $.

The limits transform as follows:
- When $ \phi = -\frac{\pi}{2} $, $ u = -1 $,
- When $ \phi = \frac{\pi}{2} $, $ u = 1 $.

The integrand simplifies to:

$$
\frac{1}{2^{3/2}} \cdot \int_{-1}^{1} (1 - u) \cdot 2 \, du = \frac{1}{2^{1/2}} \int_{-1}^{1} (1 - u) \, du.
$$

---

### Step 3: Evaluate the Integral

$$
\int_{-1}^{1} (1 - u) \, du = \left[u - \frac{u^2}{2} \right]_{-1}^{1