We wish to calculate

  I = ∫₀ᴨ cos(x + cos x) dx.

Step 1. (Using symmetry)  
Make the substitution u = π − x. Then, when x = 0, u = π and when x = π, u = 0. Also, dx = −du. Changing the variable we get

  I = ∫₀ᴨ cos(x + cos x) dx  
    = ∫π⁰ cos((π − u) + cos(π − u)) (−du)  
    = ∫₀ᴨ cos((π − u) + cos(π − u)) du.

Now note that cos(π − u) = −cos u. Therefore,
  (π − u) + cos(π − u) = (π − u) − cos u = π − (u + cos u).

Then using the cosine identity cos(π − θ) = −cos θ we have

  cos(π − (u + cos u)) = −cos(u + cos u).

Thus the transformed integral becomes

  I = ∫₀ᴨ [−cos(u + cos u)] du = −∫₀ᴨ cos(u + cos u) du.

But the integral on the right is exactly I since u is a dummy variable:

  I = −I  ⟹  2I = 0  ⟹  I = 0.

Step 2. (Conclusion)  
The exact value of the integral is 0.

Step 3. (Numerical Approximation)  
Numerically, 0 is of course 0.0000000000 when rounded to 10 decimal places.

Final Answer in JSON format:
{"answer": "$0$", "numerical_answer": "0.0000000000"}