<think>
Okay, let's see. I need to compute the definite integral from 0 to 2 of x^(1/2)(2 - x)^(1/2) cosh(1 * sqrt(x(2 - x))) dx. Hmm, that looks a bit complicated. Let me start by understanding the integrand.

First, the integrand is x^(1/2) times (2 - x)^(1/2) times the hyperbolic cosine of sqrt(x(2 - x)). Let me write that out again: √x * √(2 - x) * cosh(√(x(2 - x))). Maybe there's a substitution that can simplify this expression.

Looking at the argument inside the cosh function, it's sqrt(x(2 - x)). Let me denote that as some variable. Let's try substitution u = x(2 - x). Then du/dx = 2 - 2x. Wait, but that might not directly help. Alternatively, maybe a trigonometric substitution? Since the expression under the square root is x(2 - x), which resembles a quadratic that can be rewritten as 1 - (x - 1)^2. Let me check:

x(2 - x) = 2x - x² = -(x² - 2x) = -(x² - 2x + 1 - 1) = -(x - 1)^2 + 1. So, x(2 - x) = 1 - (x - 1)^2. That looks like a form suitable for a trigonometric substitution. Let me set x - 1 = sinθ, so that x = 1 + sinθ. Then, dx = cosθ dθ. Let's see what the limits become. When x = 0, sinθ = -1, so θ = -π/2. When x = 2, sinθ = 1, so θ = π/2. So the integral becomes from θ = -π/2 to θ = π/2.

Let's substitute. First, x = 1 + sinθ, so 2 - x = 1 - sinθ. Then sqrt(x(2 - x)) = sqrt(1 - (x - 1)^2) = sqrt(1 - sin²θ) = cosθ. So the argument of cosh is cosθ. Then the integrand becomes sqrt(x) * sqrt(2 - x) * cosh(cosθ). Let's compute sqrt(x) * sqrt(2 - x):

sqrt(x(2 - x)) = sqrt(1 - (x - 1)^2) = cosθ. So sqrt(x) * sqrt(2 - x) = cosθ. Therefore, the integrand simplifies to cosθ * cosh(cosθ). And dx is cosθ dθ. So putting it all together, the integral becomes the integral from θ = -π/2 to θ = π/2 of cosθ * cosh(cosθ) * cosθ dθ. Wait, no. Wait, let me check again.

Wait, sqrt(x) * sqrt(2 - x) is sqrt(x(2 - x)) which is sqrt(1 - (x - 1)^2) = cosθ. So that term is cosθ. Then the cosh term is cosh(cosθ). Then dx is cosθ dθ. So the entire integral becomes:

∫_{-π/2}^{π/2} cosθ * cosh(cosθ) * cosθ dθ = ∫_{-π/2}^{π/2} cos²θ * cosh(cosθ) dθ.

Hmm, that's an integral over θ. Let's note that the integrand is even because cos²θ is even, cosh(cosθ) is even (since cosh is even and cosθ is even). So the integral from -π/2 to π/2 is twice the integral from 0 to π/2. So we can write 2 * ∫_{0}^{π/2} cos²θ * cosh(cosθ) dθ.

Now, how to compute this integral? Let's consider expanding cosh(cosθ) in a Taylor series. The hyperbolic cosine function can be written as a series: cosh(z) = Σ_{n=0}^∞ z^{2n}/(2n)! So substituting z = cosθ, we have cosh(cosθ) = Σ_{n=0}^∞ (cosθ)^{2n}/(2n)!.

Therefore, the integral becomes 2 * Σ_{n=0}^∞ [1/(2n)!] ∫_{0}^{π/2} cos²θ * (cosθ)^{2n} dθ = 2 * Σ_{n=0}^∞ [1/(2n)!] ∫_{0}^{π/2} cos^{2n + 2}θ dθ.

So, the integral becomes 2 * Σ_{n=0}^∞ [1/(2n)!] * ∫_{0}^{π/2} cos^{2(n + 1)}θ dθ.

The integral of cos^{2m}θ dθ from 0 to π/2 is known and is given by (π/2) * (1 * 3 * 5 * ... * (2m - 1)) / (2 * 4 * 6 * ... * 2m)) = (π/2) * ( (2m)! ) / (4^m (m!)^2 ) ). So for m = n + 1, the integral becomes (π/2) * ( (2(n + 1))! ) / (4^{n + 1} ( (n + 1)! )^2 ) ).

Therefore, substituting back into the sum:

2 * Σ_{n=0}^∞ [1/(2n)!] * (π/2) * ( (2n + 2)! ) / (4^{n + 1} ( (n + 1)! )^2 ) )

Simplify this expression. Let's factor out constants:

2 * (π/2) = π. So we have π * Σ_{n=0}^∞ [ (2n + 2)! / ( (2n)! * 4^{n + 1} ( (n + 1)! )^2 ) ) ]

Let me see if we can simplify the terms inside the summation. Let's write (2n + 2)! as (2n + 2)(2n + 1)(2n)! So:

(2n + 2)! = (2n + 2)(2n + 1)(2n)!.

Therefore, the term becomes:

(2n + 2)(2n + 1)(2n)! / [ (2n)! * 4^{n + 1} ( (n + 1)! )^2 ) ] = (2n + 2)(2n + 1) / [4^{n + 1} ( (n + 1)! )^2 ) ]

Simplify numerator and denominator:

(2n + 2)(2n + 1) = 2(n + 1)(2n + 1)

Denominator: 4^{n + 1} ( (n + 1)! )^2 = 4 * 4^n * ( (n + 1)! )^2

So the term becomes:

2(n + 1)(2n + 1) / [4 * 4^n * ( (n + 1)! )^2 ) ] = [2(n + 1)(2n + 1) ] / [4^{n + 1} ( (n + 1)! )^2 ) ]

Simplify numerator and denominator by 2:

= [ (n + 1)(2n + 1) ] / [ 2 * 4^{n} ( (n + 1)! )^2 ) ]

But (n + 1)! = (n + 1) * n!, so ( (n + 1)! )^2 = (n + 1)^2 (n! )^2. Therefore:

= [ (n + 1)(2n + 1) ] / [ 2 * 4^{n} * (n + 1)^2 (n! )^2 ) ] = [ (2n + 1) ] / [ 2 * 4^{n} * (n + 1) (n! )^2 ) ]

Hmm, this seems a bit complicated. Maybe there's a better way to approach this. Alternatively, perhaps we can reindex the sum. Let's let m = n + 1. Then when n = 0, m = 1. So the original sum is from n=0 to ∞, which becomes m=1 to ∞. But maybe that complicates things. Alternatively, let's look for known series expansions.

Alternatively, perhaps integrating term by term is not the best approach here. Let me think if there's another substitution or identity that can be used.

Wait, the integral after substitution is 2 * ∫_{0}^{π/2} cos²θ * cosh(cosθ) dθ. Let's consider expanding cosh(cosθ) into its Taylor series:

cosh(cosθ) = Σ_{k=0}^∞ (cosθ)^{2k} / (2k)!.

Therefore, the integral becomes 2 * Σ_{k=0}^∞ [1/(2k)!] ∫_{0}^{π/2} cos^{2k + 2}θ dθ.

Which is similar to what I had before. So the integral is a sum over k of terms involving integrals of cos^{2k + 2}θ. As I mentioned, these integrals can be expressed using the beta function or the double factorial.

The integral ∫_{0}^{π/2} cos^{2m}θ dθ = (π/2) * ( (2m - 1)!! ) / (2m!! ) ). Alternatively, using the formula:

∫_{0}^{π/2} cos^{2m}θ dθ = (π/2) * ( (2m)! ) / (4^m (m! )^2 )

So substituting m = k + 1, we have:

∫_{0}^{π/2} cos^{2k + 2}θ dθ = (π/2) * ( (2k + 2)! ) / (4^{k + 1} ( (k + 1)! )^2 )

Therefore, the integral becomes:

2 * Σ_{k=0}^∞ [1/(2k)!] * (π/2) * ( (2k + 2)! ) / (4^{k + 1} ( (k + 1)! )^2 )

Simplify:

2 * (π/2) = π, so:

π * Σ_{k=0}^∞ [ (2k + 2)! / ( (2k)! * 4^{k + 1} ( (k + 1)! )^2 ) ]

Let's factor out terms:

(2k + 2)! = (2k + 2)(2k + 1)(2k)!.

So substituting:

π * Σ_{k=0}^∞ [ (2k + 2)(2k + 1)(2k)! / ( (2k)! * 4^{k + 1} ( (k + 1)! )^2 ) ) ]

Cancel (2k)!:

π * Σ_{k=0}^∞ [ (2k + 2)(2k + 1) / (4^{k + 1} ( (k + 1)! )^2 ) ) ]

Factor numerator:

(2k + 2)(2k + 1) = 2(k + 1)(2k + 1)

Denominator: 4^{k + 1} ( (k + 1)! )^2 = 4 * 4^k * ( (k + 1)! )^2

So:

π * Σ_{k=0}^∞ [ 2(k + 1)(2k + 1) / (4 * 4^k * (k + 1)!^2 ) ]

Simplify constants:

2 / 4 = 1/2, so:

π * Σ_{k=0}^∞ [ (k + 1)(2k + 1) / (4^k * (k + 1)!^2 ) ) * 1/2 ]

Wait, no. Wait, 2(k + 1) in numerator and 4 in denominator gives (2(k + 1))/4 = (k + 1)/2. Wait, let's re-express:

The term becomes:

[2(k + 1)(2k + 1)] / [4^{k + 1} (k + 1)!^2] = [2(k + 1)(2k + 1)] / [4 * 4^k (k + 1)!^2] = [ (k + 1)(2k + 1) ] / [2 * 4^k (k + 1)!^2 ]

But (k + 1)! = (k + 1) * k!, so (k + 1)!^2 = (k + 1)^2 * (k! )^2. Therefore:

= [ (k + 1)(2k + 1) ] / [2 * 4^k (k + 1)^2 (k! )^2 ) ] = [ (2k + 1) ] / [2 * 4^k (k + 1) (k! )^2 ) ]

Hmm, this seems complicated. Maybe we can write (2k + 1) as something else. Alternatively, perhaps we can reindex the sum. Let me set m = k + 1. Then when k = 0, m = 1, but the original sum starts at k=0. Let's see:

If m = k + 1, then k = m - 1. So the sum becomes:

Σ_{m=1}^∞ [ (2(m - 1) + 1) ] / [2 * 4^{m - 1} (m) ( (m - 1)! )^2 ) ]

= Σ_{m=1}^∞ [ (2m - 1) ] / [2 * 4^{m - 1} m ( (m - 1)! )^2 ) ]

But this might not help. Alternatively, perhaps there's a generating function that matches this series.

Alternatively, let's look for a closed-form expression. Let's recall that the modified Bessel function of the first kind has a series representation:

I_ν(z) = Σ_{k=0}^∞ (z/2)^{2k + ν} / (k! Γ(k + ν + 1))

But I'm not sure if that's directly applicable here. Alternatively, perhaps the integral can be related to Bessel functions. Alternatively, maybe integrating using substitution.

Wait, going back to the original substitution. After substitution, the integral became 2 ∫_{0}^{π/2} cos²θ cosh(cosθ) dθ. Let's consider integrating by parts. Let u = cosθ, dv = cosh(cosθ) cosθ dθ. Hmm, not sure. Alternatively, maybe another substitution. Let t = sinθ. Then when θ = 0, t=0; θ=π/2, t=1. But not sure.

Alternatively, perhaps use the integral representation of Bessel functions. For example, the modified Bessel function I_ν(z) has an integral representation:

I_ν(z) = (1/π) ∫_{0}^π e^{z cosθ} cos(νθ) dθ

But here we have cosh(cosθ), which is (e^{cosθ} + e^{-cosθ}) / 2. So maybe we can express the integral in terms of Bessel functions.

Let me write cosh(cosθ) = (e^{cosθ} + e^{-cosθ}) / 2. Then the integral becomes:

2 * ∫_{0}^{π/2} cos²θ * [e^{cosθ} + e^{-cosθ}]/2 dθ = ∫_{0}^{π/2} cos²θ [e^{cosθ} + e^{-cosθ}] dθ

So split into two integrals:

∫_{0}^{π/2} cos²θ e^{cosθ} dθ + ∫_{0}^{π/2} cos²θ e^{-cosθ} dθ

But integrating these might be challenging. However, perhaps we can relate them to Bessel functions. Let's recall that the integral of e^{a cosθ} cos(nθ) dθ is related to modified Bessel functions. Specifically, ∫_{0}^{π} e^{a cosθ} cos(nθ) dθ = π I_n(a). But our integral is from 0 to π/2 and involves cos²θ. Let's see.

First, note that cos²θ can be written as (1 + cos2θ)/2. So:

∫_{0}^{π/2} cos²θ e^{cosθ} dθ = (1/2) ∫_{0}^{π/2} (1 + cos2θ) e^{cosθ} dθ = (1/2)[ ∫_{0}^{π/2} e^{cosθ} dθ + ∫_{0}^{π/2} cos2θ e^{cosθ} dθ ]

Similarly for the e^{-cosθ} term:

∫_{0}^{π/2} cos²θ e^{-cosθ} dθ = (1/2)[ ∫_{0}^{π/2} e^{-cosθ} dθ + ∫_{0}^{π/2} cos2θ e^{-cosθ} dθ ]

So combining both parts, the original integral becomes:

(1/2)[ ∫_{0}^{π/2} e^{cosθ} dθ + ∫_{0}^{π/2} cos2θ e^{cosθ} dθ + ∫_{0}^{π/2} e^{-cosθ} dθ + ∫_{0}^{π/2} cos2θ e^{-cosθ} dθ ]

Which simplifies to:

(1/2)[ ∫_{0}^{π/2} (e^{cosθ} + e^{-cosθ}) dθ + ∫_{0}^{π/2} cos2θ (e^{cosθ} + e^{-cosθ}) dθ ]

= (1/2)[ 2 ∫_{0}^{π/2} cosh(cosθ) dθ + 2 ∫_{0}^{π/2} cos2θ cosh(cosθ) dθ ]

= ∫_{0}^{π/2} cosh(cosθ) dθ + ∫_{0}^{π/2} cos2θ cosh(cosθ) dθ

Hmm, but this seems to complicate things further. However, perhaps we can be expressed in terms of Bessel functions. Let's recall that:

The modified Bessel function of the first kind I_n(z) has an integral representation:

I_n(z) = (1/π) ∫_{0}^{π} e^{z cosθ} cos(nθ) dθ

But our integrals are from 0 to π/2. However, note that if we extend the integral to 0 to π, we can use symmetry. For example, ∫_{0}^{π} e^{z cosθ} cos(nθ) dθ = π I_n(z). But our integral is from 0 to π/2. However, perhaps we can express the integral from 0 to π/2 in terms of Bessel functions.

Alternatively, note that:

∫_{0}^{π/2} e^{z cosθ} dθ = (1/2) ∫_{0}^{π} e^{z cosθ} dθ - (1/2) ∫_{π/2}^{π} e^{z cosθ} dθ. But since cosθ is symmetric around θ=0, the integral from 0 to π/2 is equal to the integral from π/2 to π with substitution θ → π - θ. Let me check:

Let θ' = π - θ in the integral from π/2 to π. Then cosθ' = -cosθ, and dθ' = -dθ. So:

∫_{π/2}^{π} e^{z cosθ} dθ = ∫_{0}^{π/2} e^{-z cosθ'} dθ'

Therefore, ∫_{0}^{π} e^{z cosθ} dθ = ∫_{0}^{π/2} e^{z cosθ} dθ + ∫_{0}^{π/2} e^{-z cosθ} dθ = ∫_{0}^{π/2} [e^{z cosθ} + e^{-z cosθ}] dθ = 2 ∫_{0}^{π/2} cosh(z cosθ) dθ

But from the Bessel function integral, ∫_{0}^{π} e^{z cosθ} dθ = π I_0(z). Therefore:

2 ∫_{0}^{π/2} cosh(z cosθ) dθ = π I_0(z)

So ∫_{0}^{π/2} cosh(z cosθ) dθ = (π/2) I_0(z)

Similarly, for the integral involving cos2θ:

∫_{0}^{π} e^{z cosθ} cos2θ dθ = π I_2(z)

But again, splitting into 0 to π/2 and π/2 to π:

∫_{0}^{π} e^{z cosθ} cos2θ dθ = ∫_{0}^{π/2} e^{z cosθ} cos2θ dθ + ∫_{π/2}^{π} e^{z cosθ} cos2θ dθ

Again, substitute θ' = π - θ in the second integral:

∫_{π/2}^{π} e^{z cosθ} cos2θ dθ = ∫_{0}^{π/2} e^{-z cosθ'} cos(2(π - θ')) dθ'

But cos(2π - 2θ') = cos2π cos2θ' + sin2π sin2θ' = cos2θ'

So ∫_{π/2}^{π} e^{z cosθ} cos2θ dθ = ∫_{0}^{π/2} e^{-z cosθ'} cos2θ' dθ'

Therefore, ∫_{0}^{π} e^{z cosθ} cos2θ dθ = ∫_{0}^{π/2} [e^{z cosθ} + e^{-z cosθ}] cos2θ dθ = 2 ∫_{0}^{π/2} cosh(z cosθ) cos2θ dθ

But we also have ∫_{0}^{π} e^{z cosθ} cos2θ dθ = π I_2(z). Therefore:

2 ∫_{0}^{π/2} cosh(z cosθ) cos2θ dθ = π I_2(z)

So ∫_{0}^{π/2} cosh(z cosθ) cos2θ dθ = (π/2) I_2(z)

Therefore, returning to our original integrals:

∫_{0}^{π/2} cosh(cosθ) dθ = (π/2) I_0(1)

And ∫_{0}^{π/2} cos2θ cosh(cosθ) dθ = (π/2) I_2(1)

Therefore, the original integral (after substitution) becomes:

(π/2) I_0(1) + (π/2) I_2(1) = (π/2)(I_0(1) + I_2(1))

But we need to recall that the original integral after substitution was 2 * ∫_{0}^{π/2} cos²θ cosh(cosθ) dθ, which we transformed into:

∫_{0}^{π/2} cosh(cosθ) dθ + ∫_{0}^{π/2} cos2θ cosh(cosθ) dθ = (π/2)(I_0(1) + I_2(1))

Wait, no. Wait, earlier steps: after expanding cos²θ as (1 + cos2θ)/2 and splitting the integrals, we ended up with:

Original integral after substitution was 2 * ∫_{0}^{π/2} cos²θ cosh(cosθ) dθ = ∫_{0}^{π/2} cosh(cosθ) dθ + ∫_{0}^{π/2} cos2θ cosh(cosθ) dθ

Which equals (π/2) I_0(1) + (π/2) I_2(1). Therefore, the original integral is:

(π/2)(I_0(1) + I_2(1))

But wait, no. Wait, the original integral after substitution was 2 * ∫_{0}^{π/2} cos²θ cosh(cosθ) dθ. Then we expanded cos²θ as (1 + cos2θ)/2, leading to:

2 * [ (1/2) ∫_{0}^{π/2} cosh(cosθ) dθ + (1/2) ∫_{0}^{π/2} cos2θ cosh(cosθ) dθ ] = ∫_{0}^{π/2} cosh(cosθ) dθ + ∫_{0}^{π/2} cos2θ cosh(cosθ) dθ

Which is equal to (π/2) I_0(1) + (π/2) I_2(1). Therefore, the original integral is (π/2)(I_0(1) + I_2(1)).

But we need to confirm this. Let me check:

Yes, because:

∫_{0}^{π/2} cosh(cosθ) dθ = (π/2) I_0(1)

And ∫_{0}^{π/2} cos2θ cosh(cosθ) dθ = (π/2) I_2(1)

Therefore, the sum is (π/2)(I_0(1) + I_2(1))

But wait, the modified Bessel functions have recurrence relations. For example, the relation between I_0, I_1, I_2, etc. Specifically, there's a recurrence relation:

I_{ν-1}(z) - I_{ν+1}(z) = (2ν/z) I_ν(z)

For ν=1, this gives:

I_0(z) - I_2(z) = (2*1/z) I_1(z)

So I_0(z) - I_2(z) = (2/z) I_1(z)

Therefore, I_0(z) + I_2(z) = 2 I_0(z) - (2/z) I_1(z)

Wait, maybe not helpful. Alternatively, perhaps there's a relation that can express I_0 + I_2 in terms of derivatives or something else.

Alternatively, perhaps using the modified Bessel functions' expressions. For example, I_0(1) and I_2(1) can be expressed in terms of series:

I_ν(z) = Σ_{k=0}^∞ (z/2)^{2k + ν} / (k! Γ(k + ν + 1))

For ν=0:

I_0(1) = Σ_{k=0}^∞ (1/2)^{2k} / (k! Γ(k + 1)) ) = Σ_{k=0}^∞ (1/(4^k (k!)^2))

Similarly, I_2(1) = Σ_{k=0}^∞ (1/2)^{2k + 2} / (k! Γ(k + 3)) ) = Σ_{k=0}^∞ (1/(4^{k} (k!)(k + 2)!)) ) * (1/2^2) ?

Wait, let's compute I_2(1):

I_2(1) = Σ_{k=0}^∞ (1/2)^{2k + 2} / (k! (k + 2)! )) )

= (1/2^2) Σ_{k=0}^∞ (1/4^k) / (k! (k + 2)! )

= (1/4) Σ_{k=0}^∞ 1/(4^k k! (k + 2)! )

But this might not help in simplifying I_0 + I_2. Alternatively, perhaps there's a relation between I_0 and I_2. Let's recall that:

I_ν-1(z) - I_ν+1(z) = (2ν/z) I_ν(z)

For ν=1: I_0(z) - I_2(z) = (2/z) I_1(z)

Therefore, I_0(z) + I_2(z) = 2 I_0(z) - (2/z) I_1(z)

But I don't see an immediate simplification. However, perhaps for z=1, we can write:

I_0(1) + I_2(1) = 2 I_0(1) - 2 I_1(1)

But this might not help. Alternatively, perhaps we can use another recurrence relation. For example:

I_ν-1(z) + I_ν+1(z) = 2 I_ν'(z)

But I'm not sure. Alternatively, perhaps we can use the derivative of I_0(z). The derivative of I_0(z) is I_1(z). So I_0’(z) = I_1(z). Similarly, I_1’(z) = (I_0(z) + I_2(z))/2. Wait, let's check:

The standard recurrence relations for modified Bessel functions are:

I_ν’(z) = I_{ν-1}(z) - (ν/z) I_ν(z)

And also:

I_ν’(z) = I_{ν+1}(z) + (ν/z) I_ν(z)

So combining these:

I_{ν-1}(z) - (ν/z) I_ν(z) = I_{ν+1}(z) + (ν/z) I_ν(z)

Which gives:

I_{ν-1}(z) - I_{ν+1}(z) = (2ν/z) I_ν(z)

Which is the same as before.

Alternatively, for ν=1:

I_0(z) - I_2(z) = (2/z) I_1(z)

So I_0(z) + I_2(z) = 2 I_0(z) - (2/z) I_1(z)

But unless we can express this in terms of I_0 and I_1, which might not necessarily simplify the expression.

Alternatively, perhaps the sum I_0(1) + I_2(1) can be expressed in terms of I_0(1) and I_1(1). Let's compute it numerically to see if there's a pattern.

But perhaps there's a better approach. Let's recall that the original integral after substitution is (π/2)(I_0(1) + I_2(1)). But the original integral was expressed in terms of x from 0 to 2. So the answer is (π/2)(I_0(1) + I_2(1)).

But is there a way to simplify this further? Let's recall that I_0 and I_2 are related through the recurrence. For z=1:

I_0(1) - I_2(1) = 2 I_1(1)

So I_0(1) + I_2(1) = 2 I_0(1) - 2 I_1(1)

But substituting back into the integral:

(π/2)(2 I_0(1) - 2 I_1(1)) = π (I_0(1) - I_1(1))

Wait, but this would be the case if I_0 + I_2 = 2 I_0 - 2 I_1, but according to the recurrence:

I_0 - I_2 = 2 I_1, so I_0 + I_2 = I_0 + (I_0 - 2 I_1) = 2 I_0 - 2 I_1. Yes, that's correct.

Therefore, the integral becomes (π/2)(2 I_0(1) - 2 I_1(1)) = π (I_0(1) - I_1(1))

So the original integral is π (I_0(1) - I_1(1)).

That's a simpler expression. Therefore, the exact answer is π (I_0(1) - I_1(1)).

Now, we need to verify this. Let me check the steps again.

We had:

Original integral after substitution became 2 * ∫_{0}^{π/2} cos²θ cosh(cosθ) dθ = ∫_{0}^{π/2} cosh(cosθ) dθ + ∫_{0}^{π/2} cos2θ cosh(cosθ) dθ = (π/2)(I_0(1) + I_2(1))

Then using the recurrence relation I_0 - I_2 = 2 I_1, so I_0 + I_2 = 2 I_0 - 2 I_1, so (π/2)(2 I_0 - 2 I_1) = π (I_0 - I_1). Yes, that's correct.

Therefore, the exact answer is π (I_0(1) - I_1(1)).

Now, we need to compute this numerically. Let's recall the values of the modified Bessel functions at 1.

The modified Bessel function of the first kind I_0(1) and I_1(1) have known values. Let's look them up or compute them.

The series for I_0(z) is Σ_{k=0}^∞ (z/2)^{2k} / (k!)^2. For z=1:

I_0(1) = Σ_{k=0}^∞ 1/(4^k (k!)^2 )

Similarly, I_1(1) = Σ_{k=0}^∞ (1/2)^{2k + 1} / (k! (k + 1)! )

Let's compute these numerically.

First, compute I_0(1):

I_0(1) ≈ 1 + 1/(4*1) + 1/(4^2*(2)^2) + 1/(4^3*(6)^2) + 1/(4^4*(24)^2) + ...

Calculating terms:

Term 0: 1

Term 1: 1/4 ≈ 0.25

Term 2: 1/(16*4) = 1/64 ≈ 0.015625

Term 3: 1/(64*36) ≈ 1/2304 ≈ 0.0004340277778

Term 4: 1/(256*576) ≈ 1/147456 ≈ 0.000006781684

Term 5: 1/(1024*14400) ≈ 1/14,745,600 ≈ 6.78e-8

So summing up the first few terms:

1 + 0.25 = 1.25

+ 0.015625 = 1.265625

+ 0.0004340277778 ≈ 1.2660588056

+ 0.000006781684 ≈ 1.2660655872

Further terms are negligible. The actual value of I_0(1) is approximately 1.266065878. Let's confirm with a calculator or known value. From tables, I_0(1) ≈ 1.2660658777520084.

Similarly, I_1(1):

I_1(1) = Σ_{k=0}^∞ (1/2)^{2k + 1} / (k! (k + 1)! )

= (1/2) Σ_{k=0}^∞ 1/(4^k k! (k + 1)! )

Compute terms:

Term 0: (1/2) * 1/(1*1) = 0.5

Term 1: (1/2) * 1/(4*1*2) = 1/(16) ≈ 0.0625

Term 2: (1/2) * 1/(16*2*6) = 1/(192) ≈ 0.005208333333

Term 3: (1/2) * 1/(64*6*24) = 1/(18432) ≈ 0.00005425347222

Term 4: (1/2) * 1/(256*24*120) = 1/(737280) ≈ 0.000001356481481

Summing up:

0.5 + 0.0625 = 0.5625

+ 0.005208333333 ≈ 0.5677083333

+ 0.00005425347222 ≈ 0.5677625868

+ 0.000001356481481 ≈ 0.5677639433

Further terms are negligible. The actual value of I_1(1) is approximately 0.5651591039... Wait, but my calculation here gives 0.56776, which is conflicting. Wait, perhaps I made a mistake in the calculation.

Wait, let's check the series for I_1(1):

I_1(1) = Σ_{k=0}^∞ (1/2)^{2k + 1} / (k! (k + 1)! ) )

= (1/2) Σ_{k=0}^∞ (1/4)^k / (k! (k + 1)! )

Let's compute term:

k=0: (1/2) * 1/(0! 1!) = 1/2 * 1/1 = 0.5

k=1: (1/2) * (1/4)^1 / (1! 2!) = (1/2)*(1/4)/(1*2) = (1/2)*(1/8) = 1/16 ≈ 0.0625

k=2: (1/2)*(1/4)^2 / (2! 3!) = (1/2)*(1/16)/(2*6) = (1/32)/12 = 1/384 ≈ 0.002604166667

k=3: (1/2)*(1/4)^3 / (3! 4!) = (1/2)*(1/64)/(6*24) = (1/128)/144 = 1/18432 ≈ 0.00005425347222

k=4: (1/2)*(1/4)^4 / (4! 5!) = (1/2)*(1/256)/(24*120) = (1/512)/2880 = 1/1,474,560 ≈ 6.78e-7

So summing:

0.5 + 0.0625 = 0.5625

+ 0.002604166667 ≈ 0.5651041667

+ 0.00005425347222 ≈ 0.5651584201

+ 0.000000678 ≈ 0.5651590981

So the sum converges to approximately 0.5651591. Comparing to known value, I_1(1) ≈ 0.5651591039..., which matches. So I_1(1) ≈ 0.5651591039.

Therefore, I_0(1) - I_1(1) ≈ 1.2660658778 - 0.5651591039 ≈ 0.7009067739.

Therefore, the integral is π * 0.7009067739 ≈ 2.202016621.

But let's compute this more accurately. Using more precise values:

I_0(1) ≈ 1.2660658777520084

I_1(1) ≈ 0.5651591039924853

Difference: 1.2660658777520084 - 0.5651591039924853 = 0.7009067737595231

Multiply by π: 0.7009067737595231 * π ≈ 0.7009067737595231 * 3.141592653589793 ≈ 2.2020166217064085

Rounded to 10 decimal places: 2.2020166217

But let's verify this with numerical integration to check if this is correct.

Alternatively, perhaps compute the original integral numerically using a calculator or software. But since I don't have access to that, I'll proceed with the analytical result.

Therefore, the exact answer is π (I_0(1) - I_1(1)), and the numerical approximation is approximately 2.2020166217.

But let's confirm the steps once more to ensure no mistakes.

Original integral: ∫₀² √x √(2 - x) cosh(√(x(2 - x))) dx

Substitution x = 1 + sinθ, leading to integral 2 ∫₀^{π/2} cos²θ cosh(cosθ) dθ

Expressed as π/2 (I₀(1) + I₂(1)), then using recurrence relation to get π (I₀(1) - I₁(1))

Yes, that seems correct.

Therefore, the exact answer is π (I₀(1) - I₁(1)), and the numerical value is approximately 2.2020166217.
</think>

{"answer": "\\pi \\left(I_0(1) - I_1(1)\\right)", "numerical_answer": "2.2020166217"}