# Calculating $\int_{0}^{2} x^{-1/2} (2-x)^{-1/2} [1-0.5x(2-x)]^{1} dx$

## Step 1: Analyze the integral
Let's rewrite the integral to understand its structure:
$$\int_{0}^{2} x^{-1/2} (2-x)^{-1/2} [1-0.5x(2-x)]^{1} dx$$

First, I'll expand the term $1-0.5x(2-x)$:
$$1-0.5x(2-x) = 1-0.5(2x-x^2) = 1-x+0.5x^2$$

## Step 2: Substitute variables
Let's use the substitution $x = 2\sin^2\theta$, which is helpful for integrals with this form.

When $x = 2\sin^2\theta$:
- $dx = 4\sin\theta\cos\theta\,d\theta$
- $x^{-1/2} = (2\sin^2\theta)^{-1/2} = \frac{1}{\sqrt{2}|\sin\theta|} = \frac{1}{\sqrt{2}\sin\theta}$ since $\sin\theta \geq 0$ in our range
- $(2-x)^{-1/2} = (2-2\sin^2\theta)^{-1/2} = (2\cos^2\theta)^{-1/2} = \frac{1}{\sqrt{2}|\cos\theta|} = \frac{1}{\sqrt{2}\cos\theta}$

When $x = 0$, $\sin^2\theta = 0$, so $\theta = 0$
When $x = 2$, $\sin^2\theta = 1$, so $\theta = \frac{\pi}{2}$

## Step 3: Substitute for the bracketed term
For the term $[1-0.5x(2-x)]^1$, we substitute $x = 2\sin^2\theta$:
$$1-0.5(2\sin^2\theta)(2-2\sin^2\theta) = 1-0.5(4\sin^2\theta\cos^2\theta) = 1-2\sin^2\theta\cos^2\theta = 1-\frac{1}{2}\sin^2(2\theta)$$

## Step 4: Rewrite the integral
After substitution, our integral becomes:
$$\int_{0}^{\pi/2} \frac{1}{\sqrt{2}\sin\theta} \cdot \frac{1}{\sqrt{2}\cos\theta} \cdot \left(1-\frac{1}{2}\sin^2(2\theta)\right) \cdot 4\sin\theta\cos\theta\,d\theta$$

Simplifying:
$$\int_{0}^{\pi/2} \frac{4\sin\theta\cos\theta}{\sqrt{2}\sin\theta \cdot \sqrt{2}\cos\theta} \cdot \left(1-\frac{1}{2}\sin^2(2\theta)\right) \,d\theta$$

$$\int_{0}^{\pi/2} \frac{4}{\sqrt{2} \cdot \sqrt{2}} \cdot \left(1-\frac{1}{2}\sin^2(2\theta)\right) \,d\theta$$

$$\int_{0}^{\pi/2} 2 \cdot \left(1-\frac{1}{2}\sin^2(2\theta)\right) \,d\theta$$

$$2\int_{0}^{\pi/2} \left(1-\frac{1}{2}\sin^2(2\theta)\right) \,d\theta$$

## Step 5: Evaluate the integral
$$2\int_{0}^{\pi/2} \,d\theta - \int_{0}^{\pi/2} \sin^2(2\theta) \,d\theta$$

For the first part:
$$2\int_{0}^{\pi/2} \,d\theta = 2\theta\big|_{0}^{\pi/2} = 2 \cdot \frac{\pi}{2} = \pi$$

For the second part, using the identity $\sin^2(2\theta) = \frac{1-\cos(4\theta)}{2}$:
$$\int_{0}^{\pi/2} \sin^2(2\theta) \,d\theta = \int_{0}^{\pi/2} \frac{1-\cos(4\theta)}{2} \,d\theta = \frac{1}{2}\int_{0}^{\pi/2} (1-\cos(4\theta)) \,d\theta$$

$$= \frac{1}{2}\left[\theta - \frac{\sin(4\theta)}{4}\right]_{0}^{\pi/2} = \frac{1}{2}\left[\frac{\pi}{2} - \frac{\sin(2\pi)}{4} - \left(0 - \frac{\sin(0)}{4}\right)\right]$$

$$= \frac{1}{2} \cdot \frac{\pi}{2} = \frac{\pi}{4}$$

## Step 6: Combine results
The integral equals:
$$\pi - \frac{\pi}{4} = \frac{3\pi}{4}$$

## Step 7: Numerical approximation
$\frac{3\pi}{4} \approx 2.3561944902$ (rounded to 10 decimal places)

{"answer": "\\frac{3\\pi}{4}", "numerical_answer": "2.3561944902"}