<think>
Okay, so I need to compute the definite integral of tanh(x) divided by e^x from 0 to infinity. Let me start by writing down the integral:

∫₀^∞ [tanh(x) / e^x] dx

First, I remember that tanh(x) is (e^x - e^(-x)) / (e^x + e^(-x)). Maybe substituting that in will help simplify the integrand. Let me try that substitution.

So, tanh(x) = [e^x - e^(-x)] / [e^x + e^(-x)]. Therefore, the integrand becomes:

[ (e^x - e^(-x)) / (e^x + e^(-x)) ] * e^(-x) ] = [ (e^x - e^(-x)) / (e^x + e^(-x)) ] * e^(-x)

Let me simplify this expression. Multiply numerator and denominator by e^x to make it easier. Wait, maybe not. Let's see:

First, multiply out the e^(-x):

Numerator: (e^x - e^(-x)) * e^(-x) = e^(x - x) - e^(-2x) = 1 - e^(-2x)

Denominator: (e^x + e^(-x)) = e^x + e^(-x)

So the integrand simplifies to (1 - e^(-2x)) / (e^x + e^(-x))

Hmm, maybe that's a better form. Let me check:

Wait, original integrand: tanh(x) * e^(-x) = [ (e^x - e^(-x)) / (e^x + e^(-x)) ] * e^(-x)

Multiplying numerator: (e^x - e^(-x)) * e^(-x) = e^(0) - e^(-2x) = 1 - e^(-2x)

Denominator remains e^x + e^(-x). So yes, the integrand is (1 - e^(-2x))/(e^x + e^(-x)).

Hmm, perhaps I can split the numerator into two terms:

(1)/(e^x + e^(-x)) - e^(-2x)/(e^x + e^(-x))

So the integral becomes the integral from 0 to ∞ of [1/(e^x + e^(-x)) - e^(-2x)/(e^x + e^(-x))] dx

Let me split this into two separate integrals:

I = ∫₀^∞ [1/(e^x + e^(-x))] dx - ∫₀^∞ [e^(-2x)/(e^x + e^(-x))] dx

Let me call the first integral I1 and the second I2. So I = I1 - I2.

First, compute I1: ∫₀^∞ 1/(e^x + e^(-x)) dx

To compute I1, let's make a substitution. Let u = e^x. Then du = e^x dx, so dx = du/u.

When x = 0, u = 1; when x → ∞, u → ∞. So the integral becomes:

∫₁^∞ [1/(u + 1/u)] * (du/u) = ∫₁^∞ [1/( (u² + 1)/u )] * (du/u) = ∫₁^∞ [u/(u² + 1)] * (1/u) du = ∫₁^∞ 1/(u² + 1) du

That's the integral of 1/(u² + 1) from 1 to ∞, which is [arctan(u)] from 1 to ∞. As u approaches ∞, arctan(u) approaches π/2, and at u=1, it's π/4. So I1 = π/2 - π/4 = π/4.

Okay, so I1 = π/4.

Now, compute I2: ∫₀^∞ [e^(-2x)] / (e^x + e^(-x)) dx

Again, maybe substitution. Let me try the same substitution as before. Let u = e^x, so du = e^x dx, dx = du/u. Then when x=0, u=1; x→∞, u→∞.

Express e^(-2x) as u^(-2). The denominator is u + 1/u. So the integrand becomes:

[u^(-2)] / [u + 1/u] * (du/u) = [1/(u²)] / [(u² + 1)/u] * (du/u) = [1/(u²)] * [u/(u² + 1)] * (du/u) = [1/(u²)] * [u/(u² + 1)] * (1/u) du

Simplify step by step:

First, denominator: u + 1/u = (u² +1)/u. So 1/(denominator) = u/(u² +1). Then multiply by e^(-2x) which is u^(-2), and dx is du/u.

So putting it all together:

u^(-2) * [u/(u² +1)] * (du/u) = u^(-2) * u * (u² +1)^(-1) * u^(-1) du

Wait, exponents: u^(-2) * u = u^(-1), then times u^(-1) is u^(-2). So:

u^(-2) / (u² +1) du

Therefore, I2 = ∫₁^∞ [1/(u²(u² +1))] du

Hmm, this integral. Let's see. Maybe partial fractions. Let's decompose 1/(u²(u² +1)).

Let me write 1/(u²(u² +1)) = A/u² + B/(u² +1). Wait, but that might not work because the denominator is u² and u² +1. Alternatively, perhaps write as (A u + B)/u² + (C u + D)/(u² +1). But maybe a different approach.

Alternatively, note that 1/(u²(u² +1)) = 1/u² - 1/(u² +1). Let me check:

1/u² - 1/(u² +1) = [ (u² +1) - u² ] / [u²(u² +1) ] = 1 / [u²(u² +1) ]

Yes, exactly. So that's correct. Therefore, 1/(u²(u² +1)) = 1/u² - 1/(u² +1). Therefore, the integral I2 becomes:

∫₁^∞ [1/u² - 1/(u² +1)] du = ∫₁^∞ 1/u² du - ∫₁^∞ 1/(u² +1) du

Compute each integral:

First integral: ∫1/u² du = -1/u. Evaluated from 1 to ∞: [-1/u] from 1 to ∞ = 0 - (-1/1) = 1.

Second integral: ∫1/(u² +1) du = arctan(u). Evaluated from 1 to ∞: π/2 - π/4 = π/4.

Therefore, I2 = 1 - π/4.

So now, going back to the original integral I = I1 - I2 = π/4 - (1 - π/4) = π/4 -1 + π/4 = π/2 -1.

Wait, the integral I is π/2 -1. So the exact answer is π/2 -1.

Now, let's check this result. Let me compute the numerical approximation. π is approximately 3.1415926536, so π/2 is about 1.5707963268. Then subtract 1, so 1.5707963268 -1 = 0.5707963268. Rounded to 10 decimal places, that's approximately 0.5707963268.

But let me verify this with another method to be sure. Alternatively, maybe I can compute the integral numerically to check.

Alternatively, let's consider another approach. Let me write the original integral as ∫₀^∞ tanh(x) e^{-x} dx.

Another way to compute this integral is to express tanh(x) as 1 - 2/(e^{2x} +1). Let me recall that tanh(x) = 1 - 2/(e^{2x} +1). Let me verify:

tanh(x) = (e^x - e^{-x})/(e^x + e^{-x}) = [e^{2x} -1]/[e^{2x} +1] = 1 - 2/(e^{2x} +1). Yes, that's correct.

So substituting into the integral:

∫₀^∞ [1 - 2/(e^{2x} +1)] e^{-x} dx = ∫₀^∞ e^{-x} dx - 2 ∫₀^∞ e^{-x}/(e^{2x} +1) dx

First integral: ∫₀^∞ e^{-x} dx = 1.

Second integral: 2 ∫₀^∞ e^{-x}/(e^{2x} +1) dx. Let me make substitution here. Let u = e^x, so du = e^x dx, dx = du/u. When x=0, u=1; x→∞, u→∞. Then e^{-x} = 1/u, and e^{2x} = u². So the integral becomes:

2 ∫₁^∞ (1/u) / (u² +1) * (du/u) = 2 ∫₁^∞ 1/(u²(u² +1)) du

Wait, this is similar to the previous I2. Wait, but in the first approach, we had I2 = 1 - π/4. But here, the second integral is 2 times that integral, which would be 2*(1 - π/4). Therefore, the original integral becomes 1 - 2*(1 - π/4) = 1 -2 + π/2 = π/2 -1. Which matches the previous result. So that's a good check.

Therefore, the exact answer is indeed π/2 -1.

Now, let's compute the numerical value. π is approximately 3.141592653589793. So π/2 is 1.5707963267948966. Subtract 1 gives approximately 0.5707963267948966. Rounded to 10 decimal places, that's 0.5707963268.

Alternatively, let me compute it using numerical integration. Let's approximate the integral ∫₀^∞ tanh(x) e^{-x} dx numerically. Since integrating from 0 to infinity, perhaps substitute x = -ln(t), but maybe just take a large upper limit.

But since we already have the analytical methods confirming π/2 -1, and the numerical approximation is about 0.5707963268, I can be confident that's correct.

So the final answer is π/2 -1, and the numerical approximation is approximately 0.5707963268.
</think>

{"answer": "\\frac{\\pi}{2} - 1", "numerical_answer": "0.5707963268"}