We wish to evaluate

  I = ∫₀¹ ((x − 1)/((x + 1) ln x)) dx.

Step 1. Expressing (x − 1)/ln x as an Integral

For x > 0, there is the useful identity
  (xᵃ − 1)/ln x = ∫₀ᵃ xᵗ dt.
Taking a = 1, we have
  (x − 1)/ln x = ∫₀¹ xᵗ dt.
Thus, the given integral becomes
  I = ∫₀¹ [1/(x + 1)] * [(x − 1)/ln x] dx
    = ∫₀¹ [1/(x + 1)] (∫₀¹ xᵗ dt) dx.
Interchange the order of integration (Fubini’s Theorem applies here):
  I = ∫₀¹ (∫₀¹ xᵗ/(x + 1) dx) dt.

Step 2. Evaluate the Inner Integral

Define for a fixed t,
  I(t) = ∫₀¹ xᵗ/(x + 1) dx.
Notice that on x ∈ [0, 1] we can use the expansion valid for |x| < 1:
  1/(x + 1) = Σₙ₌₀∞ (−1)ⁿ xⁿ.
Thus,
  I(t) = ∫₀¹ xᵗ Σₙ₌₀∞ (−1)ⁿ xⁿ dx = Σₙ₌₀∞ (−1)ⁿ ∫₀¹ x^(t+n) dx.
Since ∫₀¹ x^(t+n) dx = 1/(t + n + 1), we obtain
  I(t) = Σₙ₌₀∞ (−1)ⁿ/(t + n + 1).

Step 3. Interchange the Sum and t-Integral

Returning to I, we now have
  I = ∫₀¹ I(t) dt = ∫₀¹ Σₙ₌₀∞ (−1)ⁿ/(t + n + 1) dt.
Interchange sum and integral:
  I = Σₙ₌₀∞ (−1)ⁿ ∫₀¹ 1/(t + n + 1) dt.
We now evaluate the inner t-integral:
  ∫₀¹ 1/(t + n + 1) dt = [ln(t + n + 1)]ₜ₌₀¹ = ln((n + 2)/(n + 1)).
Thus,
  I = Σₙ₌₀∞ (−1)ⁿ ln((n + 2)/(n + 1)).

Step 4. Rewrite the Sum as a Telescoping Product

Write the sum as
  I = Σₙ₌₀∞ (−1)ⁿ [ln(n + 2) − ln(n + 1)].
Changing the index in the first sum (let m = n + 1) leads to
  I = Σₘ₌₁∞ (−1)^(m−1) ln((m + 1)/m).

We now express this alternating sum as a logarithm of an infinite product:
  I = ln(∏ₘ₌₁∞ ((m + 1)/m)^( (−1)^(m−1) )).

Let’s compute the product term‐by‐term:
  For m = 1: ((2)/1)^(+1) = 2,
  For m = 2: ((3)/2)^(−1) = 2/3,
  For m = 3: ((4)/3)^(+1) = 4/3,
  For m = 4: ((5)/4)^(−1) = 4/5,
  … and so on.

Group the terms in pairs (m = 2k − 1 and m = 2k):
  Their contribution is
   ((2k)/(2k − 1)) * ((2k)/(2k + 1)) = (4k²)/((2k − 1)(2k + 1)) = 4k²/(4k² − 1).

Thus the entire infinite product becomes
  P = ∏ₖ₌₁∞ (4k²/(4k² − 1)).
A classical product evaluation (related to Wallis’ product) shows that
  ∏ₖ₌₁∞ (4k²/(4k² − 1)) = π/2.
It follows that the original sum is
  I = ln(P) = ln(π/2).

Step 5. Numerical Approximation

We have the exact answer
  I = ln(π/2).
The numerical value is
  π/2 ≈ 1.5707963268,
  so ln(π/2) ≈ 0.4515827053 (rounded to 10 decimal places).

Final Answer in JSON Format:
{"answer": "\\ln\\frac{\\pi}{2}", "numerical_answer": "0.4515827053"}