We start with the integral

  I = ∫₋₁⁰ 5 (x⁶ + x)⁴ dx.

Step 1. Recognize that we can expand (x⁶ + x)⁴ using the binomial theorem:
  (x⁶ + x)⁴ = Σ (j = 0 to 4) [C(4, j) (x⁶)ʲ (x)^(4 – j)] = Σ (j = 0 to 4) [C(4, j) x^(6j + 4 – j)].
Since 6j + 4 – j = 5j + 4, we have
  (x⁶ + x)⁴ = Σ (j = 0 to 4) C(4, j) x^(5j + 4).

Thus the integrand becomes
  5 (x⁶ + x)⁴ = 5 Σ (j = 0 to 4) C(4, j) x^(5j + 4).

Step 2. Integrate term‐by‐term:
  I = 5 Σ (j = 0 to 4) C(4, j) ∫₋₁⁰ x^(5j + 4) dx.
The antiderivative of x^(5j + 4) is x^(5j + 5)/(5j + 5), so
  I = 5 Σ (j = 0 to 4) [C(4, j)/(5j + 5)] [ x^(5j + 5) ] evaluated from x = –1 to 0.

At the upper limit x = 0 all terms vanish. At the lower limit x = –1 we have
  x^(5j + 5) = (–1)^(5j + 5).
Notice that (–1)^(5j + 5) = (–1)^(5 (j + 1)) = [ (–1)^5 ]^(j + 1) = (–1)^(j + 1).

Thus the contribution from each term is:
  5 * C(4, j)/(5j + 5) * (0 – (–1)^(5j + 5)) = –5 * C(4, j)/(5j + 5) (–1)^(j + 1).

Factor out the 5/5 from the denominator (since 5j + 5 = 5 (j + 1)):
  I = – Σ (j = 0 to 4) [C(4, j)/(j + 1)] (–1)^(j + 1).

We can bring the minus sign inside by writing –(–1)^(j + 1) = (–1)^(j):
  I = Σ (j = 0 to 4) [C(4, j)/(j + 1)] (–1)^j.

Step 3. Compute the sum term‐by‐term:
  For j = 0: (–1)^0/(0 + 1)·C(4, 0) = 1/1 · 1 = 1.
  For j = 1: (–1)^1/(1 + 1)·C(4, 1) = (–1)/2 · 4 = –2.
  For j = 2: (–1)^2/(2 + 1)·C(4, 2) = 1/3 · 6 = 2.
  For j = 3: (–1)^3/(3 + 1)·C(4, 3) = (–1)/4 · 4 = –1.
  For j = 4: (–1)^4/(4 + 1)·C(4, 4) = 1/5 · 1 = 1/5.

Now sum them:
  1 – 2 + 2 – 1 + 1/5 = (1 – 2) + (2 – 1) + 1/5 = (–1) + 1 + 1/5 = 1/5.

Thus the exact value of the integral is
  I = 1/5.

Step 4. Numerical approximation:
  1/5 = 0.2, and rounded to 10 decimal places this is 0.2000000000.

Final Answer in JSON format:
{"answer": "\\frac{1}{5}", "numerical_answer": "0.2000000000"}