Let's begin by computing the definite integral:

\[
\int_{0}^{6} \left[ x + (x-3)^7 + \sin(x-3) \right] dx
\]

We'll split it into three parts:

\[
I = \int_{0}^{6} x \, dx + \int_{0}^{6} (x-3)^7 dx + \int_{0}^{6} \sin(x-3) dx
\]

---

### 1. \( \int_0^6 x \, dx \)

This is straightforward:

\[
\int x \, dx = \frac{x^2}{2} \implies \left[\frac{x^2}{2}\right]_0^6 = \frac{36}{2} - 0 = 18
\]

---

### 2. \( \int_0^6 (x-3)^7 dx \)

Let \( u = x - 3 \implies x = u + 3 \), so when \( x=0,\, u=-3 \) and when \( x=6,\, u=3 \):

\[
\int_{x=0}^{x=6} (x-3)^7 dx = \int_{u=-3}^{u=3} u^7 du
\]

The antiderivative of \( u^7 \) is \( \frac{u^8}{8} \):

\[
\left[ \frac{u^8}{8} \right]_{-3}^3 = \frac{3^8}{8} - \frac{(-3)^8}{8}
\]

But \( 3^8 = (-3)^8 \), so this evaluates to zero:

\[
\frac{6561}{8} - \frac{6561}{8} = 0
\]

---

### 3. \( \int_0^6 \sin(x-3) dx \)

Let \( v = x-3 \implies x = v+3 \), so when \( x=0,\, v=-3 \) and when \( x=6,\, v=3 \):

\[
\int_{x=0}^{x=6} \sin(x-3) dx = \int_{v=-3}^{v=3} \sin(v) dv
\]

The antiderivative of \( \sin(v) \) is \( -\cos(v) \):

\[
\left[ -\cos(v) \right]_{-3}^{3} = -\cos(3) + \cos(-3)
\]

But \( \cos \) is even, so \( \cos(-3) = \cos(3) \):

\[
-\cos(3) + \cos(3) = 0
\]

---

### Summing up

\[
I = 18 + 0 + 0 = 18
\]

---

### 4. Numerical Approximation

The answer is exactly 18. Rounded to 10 decimal places: **18.0000000000**

---

```json
{"answer": "18", "numerical_answer": "18.0000000000"}
```