To solve the definite integral \(\int_{-1}^1 \frac{\cos x}{1 + e^{-\frac{1}{x}}} \, dx\), we will follow the steps outlined:

### Step 1: Analytical Solution

First, let's analyze the integrand \(\frac{\cos x}{1 + e^{-\frac{1}{x}}}\). Notice that the function \(e^{-\frac{1}{x}}\) has a singularity at \(x = 0\). However, the integrand is well-behaved because \(\cos x\) is continuous and bounded.

To simplify the integral, we can use the symmetry of the integrand. Consider the substitution \(u = -x\). Then \(du = -dx\), and the limits of integration change from \(x = -1\) to \(x = 1\) to \(u = 1\) to \(u = -1\). Thus, the integral becomes:

\[
\int_{-1}^1 \frac{\cos x}{1 + e^{-\frac{1}{x}}} \, dx = \int_{1}^{-1} \frac{\cos(-u)}{1 + e^{\frac{1}{u}}} (-du) = \int_{-1}^1 \frac{\cos u}{1 + e^{\frac{1}{u}}} \, du
\]

Since \(\cos(-u) = \cos u\), we have:

\[
\int_{-1}^1 \frac{\cos x}{1 + e^{-\frac{1}{x}}} \, dx = \int_{-1}^1 \frac{\cos x}{1 + e^{\frac{1}{x}}} \, dx
\]

Now, let's add the original integral and the transformed integral:

\[
I = \int_{-1}^1 \frac{\cos x}{1 + e^{-\frac{1}{x}}} \, dx
\]
\[
I = \int_{-1}^1 \frac{\cos x}{1 + e^{\frac{1}{x}}} \, dx
\]

Adding these two integrals, we get:

\[
2I = \int_{-1}^1 \left( \frac{\cos x}{1 + e^{-\frac{1}{x}}} + \frac{\cos x}{1 + e^{\frac{1}{x}}} \right) \, dx
\]

Notice that:

\[
\frac{1}{1 + e^{-\frac{1}{x}}} + \frac{1}{1 + e^{\frac{1}{x}}} = 1
\]

Thus:

\[
2I = \int_{-1}^1 \cos x \, dx
\]

The integral of \(\cos x\) from \(-1\) to \(1\) is:

\[
\int_{-1}^1 \cos x \, dx = \sin x \Big|_{-1}^1 = \sin 1 - \sin(-1) = \sin 1 + \sin 1 = 2 \sin 1
\]

Therefore:

\[
2I = 2 \sin 1 \implies I = \sin 1
\]

### Step 2: Numerical Approximation

Using a calculator or numerical software, we find:

\[
\sin 1 \approx 0.8414709848
\]

### Step 3: JSON Output

The final answer in the required JSON format is:

```json
{"answer": "\\sin 1", "numerical_answer": "0.8414709848"}
```