

To solve the definite integral \(\int_{-1}^1 \frac{1}{3^x + 1} \, dx\), we use a symmetry substitution technique.

### Step 1: Define the integral and apply substitution
Let \( I = \int_{-1}^1 \frac{1}{3^x + 1} \, dx \). Consider the substitution \( u = -x \), which implies \( du = -dx \). When \( x = -1 \), \( u = 1 \), and when \( x = 1 \), \( u = -1 \). Rewriting the integral in terms of \( u \):

\[
I = \int_{1}^{-1} \frac{1}{3^{-u} + 1} (-du) = \int_{-1}^1 \frac{1}{3^{-u} + 1} \, du
\]

Since the variable of integration is a dummy variable, we replace \( u \) with \( x \):

\[
I = \int_{-1}^1 \frac{1}{3^{-x} + 1} \, dx
\]

### Step 2: Simplify the integrand
Note that \( 3^{-x} = \frac{1}{3^x} \), so:

\[
\frac{1}{3^{-x} + 1} = \frac{1}{\frac{1}{3^x} + 1} = \frac{3^x}{1 + 3^x}
\]

Thus, the integral becomes:

\[
I = \int_{-1}^1 \frac{3^x}{3^x + 1} \, dx
\]

### Step 3: Add the original and substituted integrals
We now have two expressions for \( I \):

\[
I = \int_{-1}^1 \frac{1}{3^x + 1} \, dx \quad \text{and} \quad I = \int_{-1}^1 \frac{3^x}{3^x + 1} \, dx
\]

Adding these two equations:

\[
2I = \int_{-1}^1 \left( \frac{1}{3^x + 1} + \frac{3^x}{3^x + 1} \right) dx
\]

The integrand simplifies to:

\[
\frac{1 + 3^x}{3^x + 1} = 1
\]

Thus:

\[
2I = \int_{-1}^1 1 \, dx = 2
\]

### Step 4: Solve for \( I \)
Dividing both sides by 2 gives \( I = 1 \).

### Numerical Approximation
The exact value is \( 1 \), so the numerical approximation to 10 decimal places is \( 1.0000000000 \).

{"answer": "1", "numerical_answer": "1.0000000000"}