We will show that the integral

  I = ∫₀² x^(1/2) (2-x)^(1/2) cos[√(x(2-x))] dx

can be written in closed‐form in terms of Bessel functions.

Step 1. Change of Variable

Notice that
  √(x(2-x)) = √(2x-x²) = √(1 - (x-1)²)
so it is natural to set

  u = x - 1,   ⇒ x = 1 + u  and dx = du,
with u going from –1 (when x = 0) to 1 (when x = 2). Also,
  x^(1/2)(2-x)^(1/2) = √((1+u)(1-u)) = √(1-u²),
and the argument in the cosine becomes
  √(x(2-x)) = √(1-u²).

Thus the integral becomes
  I = ∫₋₁¹ √(1-u²) cos(√(1-u²)) du.

Since the integrand is even (both √(1-u²) and cos(√(1-u²)) are even functions) we can write

  I = 2 ∫₀¹ √(1-u²) cos(√(1-u²)) du.

Step 2. A Trigonometric Change

A standard substitution is to let

  u = cosθ   with du = -sinθ dθ.
When u goes from 0 to 1 the angle θ goes from θ = π/2 (since cos(π/2)=0) to θ = 0 (since cos0=1). Also, note that
  √(1-u²) = √(1-cos²θ) = sinθ,   (since sinθ ≥ 0 for θ in [0,π/2]).

Thus
  I = 2 ∫_{θ=π/2}^{θ=0} sinθ cos(sinθ) (du).
But with du = -sinθ dθ we have:
  I = 2 ∫_{π/2}^{0} sinθ cos(sinθ) (– sinθ dθ)
     = 2 ∫₀^{π/2} sin²θ cos(sinθ) dθ.

It turns out that writing the whole integral over [0,π] is even more convenient. In fact, one may also show (by using the substitution x = 1 + cosθ with θ from 0 to π) that

  I = ∫₀^{π} sin²θ cos(sinθ) dθ.

Step 3. Expressing the Result via a Bessel Function

Now, define the function
  F(a) = ∫₀^{π} cos(a sinθ) dθ.
It is a standard result that
  F(a) = π J₀(a),
where J₀ is the Bessel function of order 0.

Differentiate F(a) twice with respect to a. Note that
  F''(a) = –∫₀^{π} sin²θ cos(a sinθ)dθ.
In particular, at a = 1 we have
  ∫₀^{π} sin²θ cos(sinθ)dθ = –F''(1).
Thus
  I = –F''(1) = –π J₀''(1).

Now, using the Bessel differential equation for J₀:
  z² J₀''(z) + z J₀'(z) + z² J₀(z) = 0,
we solve for J₀''(z):
  J₀''(z) = –[J₀'(z)/z + J₀(z)].
Inserting z = 1 gives
  J₀''(1) = –[J₀'(1) + J₀(1)].
Therefore,
  I = –π J₀''(1) = π [J₀'(1) + J₀(1)].

But a known relation for Bessel functions is
  J₀'(z) = –J₁(z),
so that
  J₀'(1) = –J₁(1).
Thus the final exact answer becomes

  I = π [J₀(1) – J₁(1)].

Step 4. Numerical Evaluation

Using standard approximate values:
  J₀(1) ≈ 0.7651976866  and  J₁(1) ≈ 0.4400505857,
we have
  J₀(1) – J₁(1) ≈ 0.7651976866 – 0.4400505857 = 0.3251471009.
Multiplying by π:
  I ≈ π × 0.3251471009 ≈ 1.0210176923.

Thus, the final answer is:

{"answer": "$\\pi\\left(J_0(1)-J_1(1)\\right)$", "numerical_answer": "1.0210176923"}