We begin with the given integral

  I = ∫₀² [x^(–1/2) (2 – x)^(–1/2) / √(1 + x(2 – x))] · T₃(√(1 + x(2 – x))) dx

where T₃ is the Chebyshev polynomial of degree 3. Recall that one can express the Chebyshev polynomial by

  Tₙ(z) = cos(n arccos z)

so in particular

  T₃(z) = 4z³ – 3z.

Thus, writing
  T₃(√(1 + x(2 – x))) = 4·[√(1 + x(2 – x))]³ – 3·√(1 + x(2 – x))
              = 4(1 + x(2 – x))^(3/2) – 3(1 + x(2 – x))^(1/2),

the integrand becomes

  [x^(–1/2)(2 – x)^(–1/2)] / √(1 + x(2 – x)) · {4(1 + x(2 – x))^(3/2) – 3(1 + x(2 – x))^(1/2)}.

Notice that the factors of √(1 + x(2 – x)) cancel as follows:
  4(1 + x(2 – x))^(3/2) / √(1 + x(2 – x)) = 4(1 + x(2 – x))
  and 3(1 + x(2 – x))^(1/2) / √(1 + x(2 – x)) = 3.

Thus the integrand simplifies to

  x^(–1/2)(2 – x)^(–1/2) [4(1 + x(2 – x)) – 3].

Expanding the bracket,
  4(1 + x(2 – x)) – 3 = 4 + 4x(2 – x) – 3 = 1 + 4x(2 – x).

So the integral becomes

  I = ∫₀² x^(–1/2)(2 – x)^(–1/2)[1 + 4x(2 – x)] dx.

A convenient substitution is x = 2 sin²θ. Compute the derivatives and new factors:

1. When x = 2 sin²θ then dx = 4 sinθ cosθ dθ.
2. Also, 
  x^(–1/2) = 1/√(2 sin²θ) = 1/(√2 sinθ),
  2 – x = 2 – 2 sin²θ = 2 cos²θ ⟹ (2 – x)^(–1/2) = 1/(√2 cosθ).

Thus, the product x^(–1/2)(2 – x)^(–1/2) is

  1/(√2 sinθ) · 1/(√2 cosθ) = 1/(2 sinθ cosθ).

The differential dx gives 4 sinθ cosθ dθ, so the combination yields

  x^(–1/2)(2 – x)^(–1/2) dx = [1/(2 sinθ cosθ)]·[4 sinθ cosθ dθ] = 2 dθ.

Next, we substitute into the factor 1 + 4x(2 – x). With x = 2 sin²θ and 2 – x = 2 cos²θ, we have

  x(2 – x) = (2 sin²θ)(2 cos²θ) = 4 sin²θ cos²θ.

Then

  1 + 4x(2 – x) = 1 + 4·(4 sin²θ cos²θ) = 1 + 16 sin²θ cos²θ.

Recognize that sin²(2θ) = 4 sin²θ cos²θ so that

  16 sin²θ cos²θ = 4 sin²(2θ).

Thus the integrand simplifies further to

  1 + 4 sin²(2θ).

The limits transform as follows: when x = 0, then sin²θ = 0 so θ = 0; when x = 2, then sin²θ = 1 so θ = π/2.

Thus, the integral becomes

  I = 2 ∫₀^(π/2) [1 + 4 sin²(2θ)] dθ.

We now separate the integral:

  I = 2 { ∫₀^(π/2) 1 dθ + 4 ∫₀^(π/2) sin²(2θ)dθ }.

The first integral is straightforward:

  ∫₀^(π/2) 1 dθ = π/2.

For the second, recall that

  ∫ sin²(αθ)dθ = θ/2 – sin(2αθ)/(4α) + C.
With α = 2, we get

  ∫₀^(π/2) sin²(2θ)dθ = [θ/2 – sin(4θ)/8]₀^(π/2) = (π/2)/2 – [sin(2π)/8 – sin(0)/8] = π/4.

Substituting back:

  I = 2 { (π/2) + 4·(π/4) } = 2 { (π/2) + π } = 2 · (3π/2) = 3π.

Thus the exact value of the integral is 3π.

Numerically, using π ≈ 3.141592653589793, we have

  3π ≈ 9.4247779608.

{"answer": "3\\pi", "numerical_answer": "9.4247779608"}