<think>
Okay, let's tackle this integral step by step. The integral given is ∫₀² x^(1/2) (2 - x)^(-1/2) arcsin(0.5√(x(2 - x))) dx. Hmm, that looks a bit complicated, but maybe there's a substitution that can simplify it.

First, let me rewrite the integral for clarity:
∫₀² √x / √(2 - x) * arcsin( (1/2)√(x(2 - x)) ) dx

Looking at the integrand, there's an arcsin function with an argument involving √(x(2 - x)). Maybe a trigonometric substitution would work here. Let me think about possible substitutions. The expression inside the arcsin is (1/2)√(x(2 - x)). Let's denote that as sinθ, since arcsin of something suggests that substitution. So, set:

(1/2)√(x(2 - x)) = sinθ

Then, arcsin( (1/2)√(x(2 - x)) ) = θ. That might simplify the integral. Let's try to express x in terms of θ. 

First, square both sides of the substitution:
(1/4)x(2 - x) = sin²θ
=> x(2 - x) = 4 sin²θ

But x(2 - x) is a quadratic expression. Let's see if we can express x in terms of sinθ. Let me rearrange the equation:

x(2 - x) = 4 sin²θ
=> -x² + 2x = 4 sin²θ
=> x² - 2x + 4 sin²θ = 0

Hmm, solving for x here might not be straightforward. Alternatively, maybe another substitution. Let's consider x = 2 sin²φ. Then, 2 - x = 2 - 2 sin²φ = 2 cos²φ. Let's see if that helps.

If x = 2 sin²φ, then dx = 4 sinφ cosφ dφ. Let's substitute into the integrand:

√x = √(2 sin²φ) = √2 sinφ
√(2 - x) = √(2 cos²φ) = √2 cosφ
arcsin(0.5√(x(2 - x))) = arcsin(0.5 * √(2 sin²φ * 2 cos²φ)) 
= arcsin(0.5 * √(4 sin²φ cos²φ))
= arcsin(0.5 * 2 sinφ cosφ)
= arcsin(sinφ cosφ)

Hmm, sinφ cosφ is (1/2) sin(2φ), so arcsin( (1/2) sin(2φ) ). That might complicate things. Wait, maybe there's a better substitution.

Alternatively, let's consider the substitution t = x/2. Then x = 2t, dx = 2dt, and the limits go from t=0 to t=1. Let's try that:

Integral becomes ∫₀¹ √(2t) / √(2 - 2t) * arcsin(0.5√(2t(2 - 2t))) * 2 dt

Simplify each part:

√(2t) = √2 √t
√(2 - 2t) = √2 √(1 - t)
So the first part becomes (√2 √t) / (√2 √(1 - t)) ) = √(t/(1 - t))

Inside the arcsin: 0.5√(2t * 2(1 - t)) = 0.5√(4t(1 - t)) = 0.5 * 2√(t(1 - t)) = √(t(1 - t))

So the integral becomes 2 ∫₀¹ √(t/(1 - t)) * arcsin(√(t(1 - t))) dt

Hmm, that's a bit simpler. Now, the substitution t = sin²θ. Let me try that. Let t = sin²θ, so dt = 2 sinθ cosθ dθ. When t=0, θ=0; t=1, θ=π/2.

Substituting into the integral:

2 ∫₀^{π/2} √(sin²θ / (1 - sin²θ)) * arcsin(√(sin²θ (1 - sin²θ))) * 2 sinθ cosθ dθ

Simplify:

First, √(sin²θ / cos²θ) = tanθ

Inside the arcsin: √(sin²θ cos²θ) = sinθ cosθ

So arcsin(sinθ cosθ). Hmm, sinθ cosθ = (1/2) sin(2θ), so arcsin( (1/2) sin(2θ) )

So the integral becomes 2 * 2 ∫₀^{π/2} tanθ * arcsin( (1/2) sin(2θ) ) * sinθ cosθ dθ

Simplify the constants: 4

But tanθ = sinθ / cosθ, so:

4 ∫₀^{π/2} (sinθ / cosθ) * arcsin( (1/2) sin(2θ) ) * sinθ cosθ dθ

The cosθ in the denominator cancels with the cosθ in the numerator, so:

4 ∫₀^{π/2} sin²θ * arcsin( (1/2) sin(2θ) ) dθ

Hmm, that's still complicated. Let's see if we can simplify the argument inside the arcsin. Let me denote φ = 2θ, so when θ=0, φ=0; θ=π/2, φ=π. But maybe not helpful. Alternatively, note that sin(2θ) = 2 sinθ cosθ. So (1/2) sin(2θ) = sinθ cosθ. Wait, but that's the same as before. So arcsin(sinθ cosθ). Hmm.

Alternatively, maybe another substitution. Let me set u = θ. Wait, perhaps integrating by parts. Let's consider integrating by parts, letting u = arcsin( (1/2) sin(2θ) ) and dv = sin²θ dθ. Then du would be the derivative of arcsin, and v would be the integral of sin²θ.

But integrating by parts might get messy. Let's compute du first. Let me compute the derivative of arcsin( (1/2) sin(2θ) ) with respect to θ:

d/dθ [arcsin( (1/2) sin(2θ) ) ] = [1 / √(1 - ( (1/2 sin2θ )² ))] * (1/2) * 2 cos2θ
= [1 / √(1 - (1/4 sin²2θ))] * cos2θ
Wait, let's compute it step by step:

Let f(θ) = arcsin(z), where z = (1/2) sin(2θ). Then df/dθ = (1 / √(1 - z²)) * dz/dθ

dz/dθ = (1/2) * 2 cos(2θ) = cos(2θ)

So df/dθ = cos(2θ) / √(1 - ( (1/2 sin2θ )² )

So du = [cos(2θ) / √(1 - (1/4 sin²2θ))] dθ

That seems complicated. Maybe not the best approach. Let's think differently.

Wait, perhaps there's a symmetry or a known integral. Let me check if the original integral can be related to a beta function or gamma function. The presence of x^(1/2) and (2 - x)^(-1/2) suggests that maybe a substitution to make it look like a beta function.

The beta function is ∫₀¹ t^{c-1} (1 - t)^{d-1} dt = B(c, d) = Γ(c)Γ(d)/Γ(c + d)

But our integral, after substitution t = x/2, became 2 ∫₀¹ √(t/(1 - t)) arcsin(√(t(1 - t))) dt. Hmm, but the presence of arcsin complicates things.

Alternatively, maybe express arcsin in terms of an integral. For example, arcsin(z) = ∫₀^z 1/√(1 - t²) dt. But not sure if that helps here.

Wait, let's go back to the substitution. Let me consider the substitution where we set u = √(x(2 - x)). Let me try that. Let u = √(x(2 - x)). Then u² = x(2 - x) = 2x - x². Differentiating both sides:

2u du = (2 - 2x) dx => du = (2 - 2x)/(2u) dx = (1 - x)/u dx

But not sure if that helps. Alternatively, maybe another substitution. Let me think of x = 2 sin²θ. Wait, I tried that earlier but didn't get much. Let me try again.

Set x = 2 sin²θ, so dx = 4 sinθ cosθ dθ. Then, when x = 0, θ=0; x=2, θ=π/2.

Substitute into the integral:

√x = √(2 sin²θ) = √2 sinθ

√(2 - x) = √(2 - 2 sin²θ) = √(2 cos²θ) = √2 cosθ

arcsin(0.5√(x(2 - x))) = arcsin(0.5 * √(2 sin²θ * 2 cos²θ)) = arcsin(0.5 * √(4 sin²θ cos²θ)) = arcsin(0.5 * 2 sinθ cosθ) = arcsin(sinθ cosθ)

So the integral becomes:

∫₀^{π/2} [√2 sinθ / √2 cosθ] * arcsin(sinθ cosθ) * 4 sinθ cosθ dθ

Simplify:

The √2 / √2 cancels. Then we have (sinθ / cosθ) * arcsin(...) * 4 sinθ cosθ dθ

Multiply terms:

(sinθ / cosθ) * 4 sinθ cosθ = 4 sin²θ

So integral becomes 4 ∫₀^{π/2} sin²θ * arcsin(sinθ cosθ) dθ

Hmm, still complicated. Let's focus on the arcsin(sinθ cosθ). Let me denote φ = θ, and see if there's a way to express sinθ cosθ in terms of another angle. For example, sinθ cosθ = (1/2) sin2θ. So arcsin( (1/2) sin2θ )

So the integral becomes 4 ∫₀^{π/2} sin²θ * arcsin( (1/2) sin2θ ) dθ

Let me make a substitution for the angle inside the arcsin. Let’s set φ = 2θ. Then when θ=0, φ=0; θ=π/2, φ=π. Then dφ = 2 dθ, so dθ = dφ/2. The integral becomes:

4 ∫₀^π sin²(φ/2) * arcsin( (1/2) sinφ ) * (dφ/2)

Simplify constants: 4 * (1/2) = 2

So 2 ∫₀^π sin²(φ/2) * arcsin( (1/2) sinφ ) dφ

But sin²(φ/2) = (1 - cosφ)/2, so substitute that:

2 ∫₀^π (1 - cosφ)/2 * arcsin( (1/2) sinφ ) dφ = ∫₀^π (1 - cosφ) arcsin( (1/2) sinφ ) dφ

Hmm, this might not be helpful. Alternatively, perhaps expand the arcsin in a series. Since arcsin(z) can be expressed as a power series for |z| ≤ 1. Here, (1/2) sinφ has maximum value 1/2, so it's within the radius of convergence.

The power series for arcsin(z) is z + (1/6) z^3 + (3/40) z^5 + ... So maybe integrating term by term.

But integrating term by term might be tedious, but perhaps possible. Let's try:

arcsin(z) = Σ_{n=0}^∞ ( (2n)! ) / (4^n (n!)^2 (2n + 1)) ) z^{2n + 1} }, for |z| ≤ 1.

So here, z = (1/2) sinφ. Then:

arcsin( (1/2) sinφ ) = Σ_{n=0}^∞ [ (2n)! / (4^n (n!)^2 (2n + 1)) ) ] * ( (1/2) sinφ )^{2n + 1}

= Σ_{n=0}^∞ [ (2n)! / (4^n (n!)^2 (2n + 1)) ) ] * (1/2)^{2n + 1} sin^{2n + 1}φ

= Σ_{n=0}^∞ [ (2n)! / (4^n (n!)^2 (2n + 1)) ) * 1/2^{2n + 1} ] sin^{2n + 1}φ

Simplify the coefficients:

4^n = 2^{2n}, so 1/4^n = 1/2^{2n}

Thus, coefficient becomes (2n)! / (2^{2n} (n!)^2 (2n + 1)) ) * 1/2^{2n + 1} = (2n)! / (2^{4n + 1} (n!)^2 (2n + 1)) )

So the integral becomes:

∫₀^π (1 - cosφ) * Σ_{n=0}^∞ [ (2n)! / (2^{4n + 1} (n!)^2 (2n + 1)) ) ] sin^{2n + 1}φ dφ

Interchange sum and integral (if valid):

Σ_{n=0}^∞ [ (2n)! / (2^{4n + 1} (n!)^2 (2n + 1)) ) ] ∫₀^π (1 - cosφ) sin^{2n + 1}φ dφ

Now, split the integral into two parts:

∫₀^π sin^{2n + 1}φ dφ - ∫₀^π sin^{2n + 1}φ cosφ dφ

Let's compute these integrals separately.

First integral: I₁ = ∫₀^π sin^{2n + 1}φ dφ

But for integer n ≥ 0, the integral of sin^{2n + 1}φ over [0, π] can be expressed using the beta function. The formula is:

∫₀^π sin^{k}φ dφ = 2 ∫₀^{π/2} sin^{k}φ dφ = 2 * (√π Γ((k + 1)/2) ) / (2 Γ((k + 2)/2) )

But for k = 2n + 1:

I₁ = 2 * (√π Γ(n + 1) ) / (2 Γ(n + 3/2) )) = (√π Γ(n + 1) ) / Γ(n + 3/2 )

Using the property Γ(n + 1) = n! and Γ(n + 3/2) = (2n + 1)!! / 2^{n + 1} } √π. Wait, maybe better to use the duplication formula or express in terms of factorials.

Alternatively, using the beta function:

∫₀^{π/2} sin^{2n + 1}φ dφ = (1/2) B(n + 1, 1/2) = (1/2) Γ(n + 1)Γ(1/2) / Γ(n + 3/2)

Since Γ(1/2) = √π, then:

I₁ = 2 * (1/2) Γ(n + 1)√π / Γ(n + 3/2) ) = Γ(n + 1)√π / Γ(n + 3/2 )

Similarly, Γ(n + 3/2) = (n + 1/2) Γ(n + 1/2) = (n + 1/2)(n - 1/2)...(1/2)√π

But perhaps using the relation Γ(n + 3/2) = (2n + 1)!! / 2^{n + 1} } √π

Wait, for example, Γ(1/2) = √π, Γ(3/2) = (1/2)√π, Γ(5/2) = (3/4)√π, etc. So in general:

Γ(n + 3/2) = (2n + 1)!! / 2^{n + 1} } √π

But Γ(n + 1) = n!

So substituting back into I₁:

I₁ = n! √π / [ (2n + 1)!! / 2^{n + 1} } √π ) ] = n! * 2^{n + 1} / (2n + 1)!! )

But (2n + 1)!! = (2n + 1)(2n - 1)...3*1. Also, n! * 2^{n} = (2n)!!. So 2^{n + 1} n! = 2 * 2^{n} n! = 2*(2n)!!. But (2n + 1)!! = (2n + 1)! / (2^n n! )

Wait, let's verify:

(2n + 1)!! = (2n + 1)(2n - 1)...3*1 = (2n + 1)! / (2^n n! )

Yes, because (2n + 1)! = (2n + 1)(2n)(2n - 1)...2*1 = (2n + 1)!! * 2^n n! )

Therefore, (2n + 1)!! = (2n + 1)! / (2^n n! )

So substituting back into I₁:

I₁ = n! * 2^{n + 1} / [ (2n + 1)! / (2^n n! ) ) ] = n! * 2^{n + 1} * 2^n n! / (2n + 1)! )

= 2^{2n + 1} (n! )^2 / (2n + 1)! )

So I₁ = 2^{2n + 1} (n! )^2 / (2n + 1)! )

Now, the second integral: I₂ = ∫₀^π sin^{2n + 1}φ cosφ dφ

Let’s make substitution u = sinφ, then du = cosφ dφ. When φ=0, u=0; φ=π, u=0. But the integral becomes ∫₀^0 u^{2n + 1} du = 0. Wait, because from 0 to π, sinφ goes up to 1 and back to 0, but cosφ changes sign. However, integrating from 0 to π, the integral becomes:

∫₀^{π/2} sin^{2n + 1}φ cosφ dφ + ∫_{π/2}^π sin^{2n + 1}φ cosφ dφ

In the first integral, cosφ is positive, and in the second, cosφ is negative. Let’s substitute u = sinφ in both:

First integral: u from 0 to 1, integral becomes u^{2n + 1} du = 1/(2n + 2)

Second integral: Let φ = π - t, then dφ = -dt, sin(π - t) = sin t, cos(π - t) = -cos t. So integral becomes ∫_{0}^{π/2} sin^{2n + 1}t (-cos t) (-dt) = ∫₀^{π/2} sin^{2n + 1}t cos t dt = 1/(2n + 2)

But with a negative sign from cos(π - t) = -cos t, and the integral becomes:

∫_{π/2}^π sin^{2n + 1}φ cosφ dφ = ∫₀^{π/2} sin^{2n + 1}t (-cos t) (-dt) = ∫₀^{π/2} sin^{2n + 1}t cos t dt = 1/(2n + 2)

But wait, the original second integral is:

∫_{π/2}^π sin^{2n + 1}φ cosφ dφ = ∫_{π/2}^π sin^{2n + 1}φ (-|cosφ|) dφ = -∫₀^{π/2} sin^{2n + 1}t cos t dt = -1/(2n + 2)

Wait, maybe I made a mistake here. Let me re-express:

Let’s substitute φ = π - t in the second integral:

When φ = π/2, t = π/2; φ = π, t = 0.

So ∫_{π/2}^π sin^{2n + 1}φ cosφ dφ = ∫_{π/2}^0 sin^{2n + 1}(π - t) (-sin t) (-dt)

Wait, sin(π - t) = sin t, cos(π - t) = -cos t. So:

= ∫_{0}^{π/2} sin^{2n + 1}t (-cos t) (-dt) = ∫₀^{π/2} sin^{2n + 1}t cos t dt

But the original integral is:

∫_{π/2}^π sin^{2n + 1}φ cosφ dφ = ∫_{π/2}^π sin^{2n + 1}φ cosφ dφ = ∫_{0}^{π/2} sin^{2n + 1}t (-cos t) (-dt) = ∫₀^{π/2} sin^{2n + 1}t cos t dt

But this is negative in the interval (π/2, π), so cosφ is negative there. So the integral becomes:

∫_{π/2}^π sin^{2n + 1}φ cosφ dφ = ∫_{π/2}^π sin^{2n + 1}φ (-|cosφ|) dφ = -∫_{0}^{π/2} sin^{2n + 1}t cos t) dt

Wait, this is getting confusing. Let's compute it directly:

Let’s compute I₂ = ∫₀^π sin^{2n + 1}φ cosφ dφ

Let u = sinφ, du = cosφ dφ. When φ=0, u=0; φ=π, u=0. So the integral becomes ∫₀^0 u^{2n + 1} du = 0. Wait, but this can't be right because the function isn't odd over the interval. Wait, but when φ goes from 0 to π, u goes from 0 to 1 and back to 0. So the integral splits into two parts:

∫₀^{π/2} sin^{2n + 1}φ cosφ dφ + ∫_{π/2}^π sin^{2n + 1}φ cosφ dφ

In the first integral, cosφ is positive, and in the second, cosφ is negative. Let’s compute each part:

First integral: u = sinφ, du = cosφ dφ. Limits from 0 to 1. Integral becomes ∫₀¹ u^{2n + 1} du = 1/(2n + 2)

Second integral: Let’s substitute φ = π - t, so when φ=π/2, t=π/2; φ=π, t=0. Then, sinφ = sin(π - t) = sin t, cosφ = -cos t, dφ = -dt. So the integral becomes:

∫_{π/2}^π sin^{2n + 1}φ cosφ dφ = ∫_{0}^{π/2} sin^{2n + 1}t (-cos t) (-dt) = ∫₀^{π/2} sin^{2n + 1}t cos t dt = 1/(2n + 2)

But wait, the second integral is ∫_{π/2}^π ... which becomes ∫₀^{π/2} sin^{2n + 1}t cos t dt. But since cos t is positive in [0, π/2], this integral is also 1/(2n + 2). But the original integral has cosφ which is negative in [π/2, π], so the second part is negative:

Wait, no. Let me re-express:

Original second integral: ∫_{π/2}^π sin^{2n + 1}φ cosφ dφ

With substitution φ = π - t, dφ = -dt, cosφ = -cos t, sinφ = sin t. So:

= ∫_{π/2}^0 sin^{2n + 1} t (-cos t) (-dt) = ∫₀^{π/2} sin^{2n + 1} t cos t dt

But cos t is positive in [0, π/2], so this integral is positive. However, the original integrand in the second part is sin^{2n + 1}φ cosφ, which is negative because cosφ is negative in [π/2, π]. So the integral over [π/2, π] is equal to ∫₀^{π/2} sin^{2n + 1} t cos t dt, but with a negative sign from cosφ. Wait, no:

Wait, when we substitute φ = π - t, the integral becomes:

∫_{π/2}^π sin^{2n + 1}φ cosφ dφ = ∫_{0}^{π/2} sin^{2n + 1} t (-cos t) (-dt) = ∫₀^{π/2} sin^{2n + 1} t cos t dt

The two negatives cancel, so it's positive. Therefore, the second integral is also 1/(2n + 2). Therefore, the total I₂ = 1/(2n + 2) + 1/(2n + 2) = 1/(n + 1)

Wait, that can't be right. Wait, no:

Wait, the first integral is ∫₀^{π/2} sin^{2n + 1}φ cosφ dφ = 1/(2n + 2)

The second integral after substitution is also ∫₀^{π/2} sin^{2n + 1}t cos t dt = 1/(2n + 2)

But the original second integral is ∫_{π/2}^π sin^{2n + 1}φ cosφ dφ = ∫₀^{π/2} sin^{2n + 1}t cos t dt = 1/(2n + 2)

But in the original integrand over [π/2, π], cosφ is negative, so the integral should be negative. Wait, but when we substitute, we have:

Original integrand over [π/2, π] is sin^{2n + 1}φ cosφ dφ = sin^{2n + 1}φ * (-|cosφ|) dφ

But after substitution, it becomes sin^{2n + 1}t * (-cos t) dt = sin^{2n + 1}t cos t dt, which is positive. So the integral over [π/2, π] is equal to the integral over [0, π/2] of sin^{2n + 1}t cos t dt, which is 1/(2n + 2). But since the original integrand over [π/2, π] is negative, the integral should be negative. Wait, this is confusing. Let me check with n=0:

For n=0, I₂ = ∫₀^π sinφ cosφ dφ. The integral of sinφ cosφ over 0 to π is zero, since it's an odd function around π/2. Let's compute it:

∫₀^π sinφ cosφ dφ = (1/2) ∫₀^π sin2φ dφ = (1/2)[ -cos2φ / 2 ]₀^π = (1/4)( -cos2π + cos0 ) = (1/4)( -1 + 1 ) = 0. So for n=0, I₂=0. But according to the previous calculation, it would be 1/(0 + 1) = 1, which is wrong. So there's a mistake in the previous reasoning.

Therefore, my earlier conclusion that I₂ = 1/(n + 1) is incorrect. Let's re-examine.

Let’s compute I₂ = ∫₀^π sin^{2n + 1}φ cosφ dφ

Let’s split into two intervals: [0, π/2] and [π/2, π]

First interval: u = sinφ, du = cosφ dφ. Integral becomes ∫₀¹ u^{2n + 1} du = 1/(2n + 2)

Second interval: Let φ = π - t, then sinφ = sin t, cosφ = -cos t, dφ = -dt. The integral becomes:

∫_{π/2}^π sin^{2n + 1}φ cosφ dφ = ∫_{0}^{π/2} sin^{2n + 1}t (-cos t) (-dt) = ∫₀^{π/2} sin^{2n + 1}t cos t dt = 1/(2n + 2)

But the original integrand in the second interval is sin^{2n + 1}φ cosφ = sin^{2n + 1}φ * (-|cosφ|) = - sin^{2n + 1}φ |cosφ|. So the integral over [π/2, π] is:

- ∫_{π/2}^π sin^{2n + 1}φ |cosφ| dφ = - ∫₀^{π/2} sin^{2n + 1}t cos t dt = -1/(2n + 2)

Therefore, the total I₂ = 1/(2n + 2) - 1/(2n + 2) = 0

Ah, that makes sense. So for any n, I₂ = 0. Therefore, the second part of the integral cancels out. So the original integral becomes:

Σ_{n=0}^∞ [ (2n)! / (2^{4n + 1} (n!)^2 (2n + 1)) ) ] * [ I₁ - I₂ ] = Σ_{n=0}^∞ [ (2n)! / (2^{4n + 1} (n!)^2 (2n + 1)) ) ] * I₁

But I₁ = 2^{2n + 1} (n! )^2 / (2n + 1)! )

So substituting back:

Coefficient * I₁ = [ (2n)! / (2^{4n + 1} (n! )^2 (2n + 1)) ) ] * [ 2^{2n + 1} (n! )^2 / (2n + 1)! ) ]

Simplify:

= (2n)! * 2^{2n + 1} (n! )^2 / [ 2^{4n + 1} (n! )^2 (2n + 1) (2n + 1)! ) ]

Cancel terms:

(2n)! / (2n + 1)! ) = 1/(2n + 1)

2^{2n + 1} / 2^{4n + 1} = 1/2^{2n}

So:

= 1/(2n + 1) * 1/2^{2n} * 1/(2n + 1) )

Wait, let's do it step by step:

Numerator: (2n)! * 2^{2n + 1} (n! )^2

Denominator: 2^{4n + 1} (n! )^2 (2n + 1) (2n + 1)! )

Cancel (n! )^2: numerator and denominator.

Then, numerator: (2n)! * 2^{2n + 1}

Denominator: 2^{4n + 1} (2n + 1) (2n + 1)! )

Note that (2n + 1)! = (2n + 1)(2n)! )

So denominator becomes: 2^{4n + 1} (2n + 1) (2n + 1)(2n)! )

= 2^{4n + 1} (2n + 1)^2 (2n)! )

So now, numerator / denominator = [ (2n)! * 2^{2n + 1} ] / [ 2^{4n + 1} (2n + 1)^2 (2n)! ) ]

Cancel (2n)!:

= 2^{2n + 1} / [ 2^{4n + 1} (2n + 1)^2 )

= 1 / [ 2^{2n} (2n + 1)^2 )

Therefore, each term in the sum is 1 / [ 2^{2n} (2n + 1)^2 )

So the integral becomes:

Σ_{n=0}^∞ 1 / [ 2^{2n} (2n + 1)^2 )

So the original integral (which was transformed into this sum) is equal to this sum. Therefore, the value of the integral is:

Σ_{n=0}^∞ 1 / [ 4^n (2n + 1)^2 )

Now, this series is known. Let me recall some standard series. The sum Σ_{n=0}^∞ 1/( (2n + 1)^2 ) = π²/8. But here we have an additional factor of 1/4^n.

So the sum is Σ_{n=0}^∞ [1/4^n] * [1/(2n + 1)^2 ]

This is a well-known series that can be expressed in terms of the dilogarithm function, also known as the Spence's function. Specifically, the dilogarithm function Li₂(z) = Σ_{n=1}^∞ z^n / n². But our sum starts at n=0 and has terms (1/4)^n / (2n + 1)^2.

Let’s adjust the indices to match the dilogarithm. Let’s set k = 2n + 1, but that might not help directly. Alternatively, consider:

Σ_{n=0}^∞ [1/4^n] / (2n + 1)^2 = Σ_{k=0}^∞ [1/4^k] / (2k + 1)^2

Let’s write this as Σ_{k=0}^∞ (1/4)^k / (2k + 1)^2

This can be expressed in terms of the Lerch transcendent function, but perhaps there's a closed-form expression. Alternatively, recall that:

Σ_{k=0}^∞ x^{2k + 1}/(2k + 1)^2 = (1/2) [ Li₂(x) - Li₂(-x) ]

But here we have x = 1/2. Let me check:

If we set x = 1/2, then Σ_{k=0}^∞ (1/2)^{2k + 1}/(2k + 1)^2 = (1/2) [ Li₂(1/2) - Li₂(-1/2) ]

But our sum is Σ_{k=0}^∞ (1/4)^k / (2k + 1)^2 = Σ_{k=0}^∞ (1/2)^{2k} / (2k + 1)^2 = Σ_{k=0}^∞ (1/2)^{2k} / (2k + 1)^2

Let’s = (1/2)^2 = 1/4, so the sum is Σ_{k=0}^∞ (1/4)^k / (2k + 1)^2

This can be expressed as 2 * Σ_{k=0}^∞ (1/2)^{2k + 1} / (2k + 1)^2 = 2 * (1/2) [ Li₂(1/2) - Li₂(-1/2) ] = [ Li₂(1/2) - Li₂(-1/2) ]

But let's compute Li₂(1/2) and Li₂(-1/2). Known values:

Li₂(1/2) = (π²/12) - (1/2)(ln 2)^2

Li₂(-1/2) = - (π²/12) + (1/2)(ln 2)^2

So Li₂(1/2) - Li₂(-1/2) = [ (π²/12 - (1/2)(ln2)^2 ) ] - [ -π²/12 + (1/2)(ln2)^2 ] = π²/12 - (1/2)(ln2)^2 + π²/12 - (1/2)(ln2)^2 = π²/6 - (ln2)^2

Therefore, the sum Σ_{k=0}^∞ (1/4)^k / (2k + 1)^2 = π²/6 - (ln2)^2

But wait, according to the previous step, the sum is equal to [ Li₂(1/2) - Li₂(-1/2) ] = π²/6 - (ln2)^2

Therefore, the original integral is equal to this sum, which is π²/6 - (ln2)^2

But wait, let's confirm:

The integral we were calculating was the original integral transformed into this sum, which equals π²/6 - (ln2)^2. But let's trace back the constants.

Wait, the original integral after all substitutions became:

2 ∫₀^π (1 - cosφ) arcsin( (1/2) sinφ ) dφ, which was expanded into the series and found to be equal to Σ_{n=0}^∞ 1/(4^n (2n + 1)^2 ), which equals π²/6 - (ln2)^2.

But wait, no. Wait, the sum Σ_{n=0}^∞ 1/(4^n (2n + 1)^2 ) is equal to π²/6 - (ln2)^2. Therefore, the original integral is equal to this sum. Therefore, the value of the integral is π²/6 - (ln2)^2.

But let's check the constants again. The original integral after substitution became 4 ∫₀^{π/2} sin²θ * arcsin( (1/2) sin2θ ) dθ, which after expanding into a series and integrating term by term, led to the sum Σ_{n=0}^∞ 1/(4^n (2n + 1)^2 ), which equals π²/6 - (ln2)^2.

Therefore, the exact value of the integral is π²/6 - (ln2)^2.

Now, let's compute the numerical approximation. Let's compute π²/6 and (ln2)^2.

π² ≈ 9.8696044

π²/6 ≈ 1.6449340668482264

ln2 ≈ 0.69314718056

(ln2)^2 ≈ 0.4804530139182014

Therefore, π²/6 - (ln2)^2 ≈ 1.6449340668482264 - 0.4804530139182014 ≈ 1.16448105293

Rounded to 10 decimal places: 1.1644810529

But let me verify this calculation with more precise values.

Using more precise values:

π² = 9.869604401089358

π²/6 = 1.6449340668482264

ln2 = 0.6931471805599453

(ln2)^2 = 0.4804530139182014

Subtracting: 1.6449340668482264 - 0.4804530139182014 = 1.164481052930025

Rounded to 10 decimal places: 1.1644810529

But let me check with another approach. Alternatively, compute the integral numerically to verify.

Alternatively, use substitution. Let me check with x from 0 to 2. Let's use numerical integration to approximate the value.

But since we derived the exact answer as π²/6 - (ln2)^2, and the numerical approximation is approximately 1.1644810529.

Therefore, the exact answer is π²/6 - (ln2)^2, and the numerical value is approximately 1.1644810529.
</think>

{"answer": "\\frac{\\pi^2}{6} - (\\ln 2)^2", "numerical_answer": "1.1644810529"}