To evaluate the definite integral

$$
\int_0^{2} x^{-1/4} (2 - x)^{1/4} I_0\left(1.0 \cdot \sqrt[4]{x(2 - x)}\right) \, dx,
$$

we proceed through the following steps:

---

### **Step 1: Series Expansion of the Bessel Function**

The modified Bessel function of the first kind, $ I_0(z) $, has the power series expansion:

$$
I_0(z) = \sum_{k=0}^{\infty} \frac{1}{(k!)^2} \left(\frac{z}{2}\right)^{2k}.
$$

Substituting $ z = \sqrt[4]{x(2 - x)} $, we get:

$$
I_0\left(\sqrt[4]{x(2 - x)}\right) = \sum_{k=0}^{\infty} \frac{1}{(k!)^2} \left(\frac{1}{2}\right)^{2k} \left(x(2 - x)\right)^{k/2}.
$$

---

### **Step 2: Substitution and Simplification**

We substitute this into the integral:

$$
\int_0^{2} x^{-1/4} (2 - x)^{1/4} \sum_{k=0}^{\infty} \frac{1}{(k!)^2} \left(\frac{1}{2}\right)^{2k} \left(x(2 - x)\right)^{k/2} dx.
$$

Interchanging the sum and integral (justified by uniform convergence), we get:

$$
\sum_{k=0}^{\infty} \frac{1}{(k!)^2} \left(\frac{1}{2}\right)^{2k} \int_0^{2} x^{-1/4} (2 - x)^{1/4} \left(x(2 - x)\right)^{k/2} dx.
$$

Simplifying the integrand:

$$
x^{-1/4} (2 - x)^{1/4} \left(x(2 - x)\right)^{k/2} = x^{-1/4 + k/2} (2 - x)^{1/4 + k/2}.
$$

Thus, the integral becomes:

$$
\sum_{k=0}^{\infty} \frac{1}{(k!)^2} \left(\frac{1}{2}\right)^{2k} \int_0^{2} x^{k/2 - 1/4} (2 - x)^{k/2 + 1/4} dx.
$$

---

### **Step 3: Beta Function Substitution**

We use the substitution $ x = 2t $, so $ dx = 2dt $, and the integral becomes:

$$
\sum_{k=0}^{\infty} \frac{1}{(k!)^2} \left(\frac{1}{2}\right)^{2k} \cdot 2^{k + 1} \int_0^{1} t^{k/2 - 1/4} (1 - t)^{k/2 + 1/4} dt.
$$

This is a standard Beta function:

$$
\int_0^{1} t^{a - 1} (1 - t)^{b - 1} dt = B(a, b) = \frac{\Gamma(a)\Gamma(b)}{\Gamma(a + b)}.
$$

Here, $ a = k/2 + 3/4 $, $ b = k/2 + 5/4 $, so:

$$
\int_0^{1} t^{k/2 - 1/4} (1 - t)^{k/2 + 1/4} dt = B\left(\frac{k}{2} + \frac{3}{4}, \frac{k}{2} + \frac{5}{4}\right) = \frac{\Gamma\left(\frac{k}{2} + \frac{3}{4}\right)\Gamma\left(\frac{k}{2} + \frac{5}{4}\right)}{\Gamma(k + 2)}.
$$

Putting it all together:

$$
\int_0^{2} x^{-1/4} (2 - x)^{1/4} I_0\left(\sqrt[4]{x(2 - x)}\right) dx = \sum_{k=0