We start with the integral

  I = ∫₁² (9x + 4)/(x⁵ + 3x² + x) dx.

Step 1. Factor the denominator:
  x⁵ + 3x² + x = x(x⁴ + 3x + 1).

Thus the integral becomes
  I = ∫₁² (9x + 4) / [x (x⁴ + 3x + 1)] dx.

Step 2. Use partial fractions. Write
  (9x + 4) / [x (x⁴ + 3x + 1)] = A/x + (Bx³ + Cx² + Dx + E)/(x⁴ + 3x + 1).

Multiply by the denominator:
  9x + 4 = A(x⁴ + 3x + 1) + x(Bx³ + Cx² + Dx + E).

Expanding and collecting like terms:
  = A x⁴ + 3A x + A + B x⁴ + C x³ + D x² + E x
  = (A + B)x⁴ + C x³ + D x² + (3A + E)x + A.

Now equate coefficients with 9x + 4:
• x⁴: A + B = 0  ⟹ B = –A.
• x³: C = 0.
• x²: D = 0.
• x: 3A + E = 9  ⟹ E = 9 – 3A.
• constant: A = 4.

So, A = 4, B = –4, C = 0, D = 0, and E = 9 – 12 = –3.

The decomposition becomes:
  (9x + 4)/(x (x⁴ + 3x + 1)) = 4/x + (–4x³ – 3)/(x⁴ + 3x + 1).

Step 3. Write the integral as the sum of two integrals:
  I = ∫₁² 4/x dx + ∫₁² (–4x³ – 3)/(x⁴ + 3x + 1) dx.

The first integral is easy:
  ∫₁² 4/x dx = 4 ln|x| evaluated from 1 to 2 = 4 ln2.

For the second integral, notice that the derivative of u = x⁴ + 3x + 1 is
  du/dx = 4x³ + 3.
Then, because the numerator is –(4x³ + 3), we substitute:
  Let u = x⁴ + 3x + 1, so du = (4x³ + 3) dx. Thus,
  ∫₁² (–4x³ – 3)/(x⁴ + 3x + 1) dx = –∫₁² (4x³ + 3)/(u) dx = –∫ (1/u) du.
This integrates to –ln|u|. Evaluating from x = 1 to x = 2:
  u(1) = 1⁴ + 3×1 + 1 = 5,
  u(2) = 2⁴ + 3×2 + 1 = 16 + 6 + 1 = 23.
So, the second integral equals:
  –[ln(23) – ln(5)] = ln(5/23).

Step 4. Combine both parts:
  I = 4 ln2 + ln(5/23) = ln(2⁴) + ln(5/23) = ln(16) + ln(5/23) = ln(80/23).

Step 5. Provide a numerical approximation:
  80/23 ≈ 3.478260869565217.
Thus, I ≈ ln(3.478260869565217) ≈ 1.2465324100.

Finally, the answer in JSON format is:
{"answer": "\\ln\\left(\\frac{80}{23}\\right)", "numerical_answer": "1.2465324100"}