<think>
Okay, so I need to compute the definite integral of x³ divided by (3 + 2x²) squared, from 0 to 1. Hmm, let's see. Integrals can be tricky, especially with rational functions like this. Maybe substitution will work here. Let me think about possible substitutions. The denominator is (3 + 2x²)², so maybe if I let u be 3 + 2x², then du/dx would be 4x. Wait, but the numerator is x³. Let me check that.

If u = 3 + 2x², then du = 4x dx. So, x dx would be du/4. But the numerator is x³, which is x² times x. So, maybe I can express x³ as x² * x. Then, since u = 3 + 2x², x² can be expressed in terms of u. Let's see: x² = (u - 3)/2. So substituting that in, the integral becomes:

∫ x³/(3 + 2x²)² dx = ∫ [x² * x]/(u²) dx.

But x dx is du/4, so substituting, x² is (u - 3)/2, and x dx is du/4. So putting it all together:

∫ [(u - 3)/2 * (du/4)] / u².

Wait, let me make sure. Let's break it down step by step. Let u = 3 + 2x². Then du = 4x dx, so x dx = du/4. The original integral is ∫ x³/(3 + 2x²)² dx. Let's write x³ as x² * x. Then, substitute x² = (u - 3)/2, and x dx = du/4. So the integral becomes:

∫ [(u - 3)/2 * x dx] / u².

But x dx is du/4, so substituting that in:

∫ [(u - 3)/2 * (du/4)] / u².

Wait, that seems a bit off. Let me check again. The original integral is x³ dx over (3 + 2x²)². So, x³ dx can be written as x² * x dx. Then, since u = 3 + 2x², x² = (u - 3)/2. So substituting, x² becomes (u - 3)/2, and x dx is du/4. Therefore, the integral becomes:

∫ [(u - 3)/2 * (du/4)] / u².

Wait, but the denominator is u². So putting it all together:

= ∫ [(u - 3)/2 * du/4] / u²
= (1/8) ∫ (u - 3)/u² du.

That simplifies to (1/8) ∫ [u/u² - 3/u²] du
= (1/8) ∫ [1/u - 3/u²] du.

Integrating term by term:

The integral of 1/u du is ln|u|, and the integral of 3/u² is 3*(-1/u) = -3/u. So:

= (1/8)[ln|u| + 3/u] + C.

Now substitute back u = 3 + 2x²:

= (1/8)[ln(3 + 2x²) + 3/(3 + 2x²)] + C.

Now, evaluate this from 0 to 1. Let's compute the definite integral:

At upper limit 1:

(1/8)[ln(3 + 2*1²) + 3/(3 + 2*1²)] = (1/8)[ln(5) + 3/5].

At lower limit 0:

(1/8)[ln(3 + 2*0²) + 3/(3 + 2*0²)] = (1/8)[ln(3) + 3/3] = (1/8)[ln(3) + 1].

Subtracting the lower limit from the upper limit:

(1/8)[ln(5) + 3/5 - ln(3) - 1] = (1/8)[ln(5/3) + (3/5 - 1)].

Simplify 3/5 - 1 = -2/5. So:

= (1/8)[ln(5/3) - 2/5].

So the exact answer is (1/8)(ln(5/3) - 2/5). Let me check if that's correct. Wait, let me verify the steps again to make sure.

Wait, when I substituted, the integral became (1/8) ∫ (1/u - 3/u²) du. The integral is ln|u| + 3/u. Then evaluated from u at 1 and 0. When x=1, u=5; when x=0, u=3. So the definite integral is (1/8)[ (ln5 + 3/5) - (ln3 + 1) ].

Wait, wait, when x=0, u=3, so 3/(3 + 0) = 1. So yes, the lower limit is (ln3 + 1). So the difference is (ln5 + 3/5) - (ln3 + 1) = ln(5/3) + (3/5 - 1) = ln(5/3) - 2/5. Then multiplied by 1/8. So the exact answer is (ln(5/3) - 2/5)/8. Alternatively, we can write it as (ln5 - ln3 - 2/5)/8. Either way is fine.

Now, let's compute the numerical approximation. Let's compute each part step by step.

First, compute ln(5/3). Let's find the natural logarithm of 5/3. 5/3 ≈ 1.6666666667. ln(1.6666666667) ≈ 0.5108256238.

Then subtract 2/5, which is 0.4. So 0.5108256238 - 0.4 = 0.1108256238.

Then divide by 8: 0.1108256238 / 8 ≈ 0.013853202975.

Rounded to 10 decimal places, that's approximately 0.0138532030.

Wait, let me check the exact calculation step by step to ensure accuracy.

First, compute ln(5) ≈ 1.6094379124341003

ln(3) ≈ 1.0986122886681098

So ln(5) - ln(3) ≈ 1.6094379124341003 - 1.0986122886681098 ≈ 0.5108256237669905

Then subtract 2/5 (0.4): 0.5108256237669905 - 0.4 = 0.1108256237669905

Divide by 8: 0.1108256237669905 / 8 ≈ 0.013853202970873813

Rounded to 10 decimal places: 0.01385320297. But let me check with more precise calculations.

Alternatively, using a calculator steps:

Compute ln(5/3):

5/3 ≈ 1.6666666666666667

ln(1.6666666666666667) ≈ 0.5108256237669907

Subtract 0.4: 0.5108256237669907 - 0.4 = 0.1108256237669907

Divide by 8: 0.1108256237669907 / 8 = 0.013853202970873837

So approximately 0.01385320297 when rounded to 10 decimal places. So 0.01385320297. But let's check with more precise decimal places.

Alternatively, using a calculator for the exact value:

(ln(5) - ln(3) - 0.4)/8

Compute each term:

ln(5) ≈ 1.6094379124341003

ln(3) ≈ 1.0986122886681098

So ln(5) - ln(3) = 0.5108256237669905

0.5108256237669905 - 0.4 = 0.1108256237669905

Divide by 8: 0.1108256237669905 / 8 = 0.0138532029708738125

So rounding to 10 decimal places: 0.01385320297. But wait, the 11th decimal is 3, so 0.01385320297 (since 0.0138532029708738...). Wait, 0.0138532029708738... So the 10th decimal place is the 7th after the decimal: 0.01385320297. Wait, no. Let's count:

0.0138532029708738

Decimal places:

1: 0
2: 1
3: 3
4: 8
5: 5
6: 3
7: 2
8: 0
9: 2
10:9
11:7
So rounding to 10 decimal places, the 10th is the 9 in the 9th position (since after decimal, positions are 1 to 10: 0.0 (1)1 (2)3 (3)8 (4)5 (5)3 (6)2 (7)0 (8)2 (9)9 (10)7... Wait, maybe I'm getting the positions wrong. Let me write it out:

0.0138532029708738

Breaking it down:

0.0138532029708738

Wait, perhaps I made a mistake in the initial calculation. Let me use a calculator to compute the exact value numerically.

Alternatively, perhaps I can compute the integral numerically using another method to check. Let me compute the integral from 0 to 1 of x^3/(3 + 2x²)^2 dx numerically. Let's plug in x=0 to 1.

Alternatively, use substitution again. Wait, but maybe I can use numerical approximation. Let's compute the exact value as (ln(5/3) - 2/5)/8. Let me compute this:

First, compute ln(5/3):

ln(5) ≈ 1.6094379124341003

ln(3) ≈ 1.0986122886681098

ln(5/3) = ln(5) - ln(3) ≈ 0.5108256237669905

Then subtract 2/5 = 0.4: 0.5108256237669905 - 0.4 = 0.1108256237669905

Divide by 8: 0.1108256237669905 / 8 ≈ 0.013853202970873813

So rounded to 10 decimal places, that's 0.01385320297. But when I check with a calculator, perhaps using more precise steps, maybe there's a mistake in the analytical solution. Let me verify the steps again.

Wait, when I did the substitution:

Original integral: ∫ x³/(3 + 2x²)^2 dx from 0 to 1.

Substitution: u = 3 + 2x², du = 4x dx => x dx = du/4.

Express x³ as x² * x. Then x² = (u - 3)/2. So the integral becomes:

∫ [(u - 3)/2 * x dx] / u².

But x dx is du/4, so substituting:

= ∫ [(u - 3)/2 * (du/4)] / u²

= (1/8) ∫ (u - 3)/u² du

= (1/8) ∫ (1/u - 3/u²) du

Integrate term by term:

∫1/u du = ln|u| + C

∫3/u² du = 3*(-1/u) + C = -3/u + C

So the integral is (1/8)(ln|u| + 3/u) + C

Evaluated from u=3 to u=5:

At u=5: ln5 + 3/5

At u=3: ln3 + 3/3 = ln3 + 1

Subtract: (ln5 + 3/5) - (ln3 + 1) = ln(5/3) + (3/5 - 1) = ln(5/3) - 2/5

Multiply by 1/8: (ln(5/3) - 2/5)/8

Yes, that's correct. So the exact answer is (ln(5/3) - 2/5)/8. So the numerical value is approximately 0.01385320297.

Wait, but when I compute 3/5, that's 0.6, so 3/5 -1 is -0.4, which is -2/5. So that's correct.

Alternatively, maybe there's another method to solve this integral. Let me try integration by parts. Let me see.

Let u = x², dv = x/(3 + 2x²)^2 dx.

Then du = 2x dx. To find v, integrate dv:

v = ∫ x/(3 + 2x²)^2 dx.

Let me make substitution here. Let w = 3 + 2x², dw = 4x dx => x dx = dw/4.

So ∫ x/(w)^2 dx = ∫ (1/w²) * (dw/4) = (1/4) ∫ w^{-2} dw = (1/4)(-w^{-1}) + C = -1/(4w) + C = -1/(4(3 + 2x²)) + C.

So back to integration by parts:

uv - ∫ v du = x²*(-1/(4(3 + 2x²))) - ∫ (-1/(4(3 + 2x²)))*2x dx.

Simplify:

= -x²/(4(3 + 2x²)) + (1/2) ∫ x/(3 + 2x²) dx.

Now compute the remaining integral ∫ x/(3 + 2x²) dx. Again, substitution: let z = 3 + 2x², dz = 4x dx => x dx = dz/4.

So ∫ x/(3 + 2x²) dx = ∫ (1/z) * (dz/4) = (1/4) ln|z| + C = (1/4) ln(3 + 2x²) + C.

Putting it all back:

= -x²/(4(3 + 2x²)) + (1/2)*(1/4) ln(3 + 2x²) + C

= -x²/(4(3 + 2x²)) + (1/8) ln(3 + 2x²) + C.

So the indefinite integral is:

(1/8) ln(3 + 2x²) - x²/(4(3 + 2x²)) + C.

Now evaluate from 0 to 1:

At x=1:

(1/8) ln(5) - 1/(4*5) = (1/8) ln5 - 1/20.

At x=0:

(1/8) ln(3) - 0/(4*3) = (1/8) ln3.

Subtracting:

(1/8 ln5 - 1/20) - (1/8 ln3) = 1/8 (ln5 - ln3) - 1/20.

Which is the same as (ln(5/3)/8 - 1/20). Wait, but earlier we had (ln(5/3) - 2/5)/8. Let's see if these are the same.

(ln(5/3) - 2/5)/8 = (ln5 - ln3 - 2/5)/8.

But the integration by parts result is (ln5 - ln3)/8 - 1/20.

So let's see if these are equal:

(ln5 - ln3)/8 - 1/20 = (ln5 - ln3)/8 - (2/5)/8 * (8/20) ?

Wait, 1/20 is equal to 2/40, which is 1/20. Let's compute (ln5 - ln3)/8 - 1/20.

But 1/20 is 0.05, and (ln5 - ln3)/8 is approximately 0.5108256237669905 /8 ≈ 0.06385320297. Then subtract 0.05: 0.06385320297 - 0.05 = 0.01385320297, which matches the previous result. So yes, both methods give the same numerical result. Therefore, the exact answer is (ln(5/3) - 2/5)/8, which is equivalent to (ln5 - ln3)/8 - 1/20.

So the exact answer is correct. Now, to present the exact answer in LaTeX, it would be \frac{1}{8}\left( \ln\left( \frac{5}{3} \right) - \frac{2}{5} \right).

Alternatively, combining the terms over a common denominator, but perhaps the simplest form is as written.

So the final answer in JSON should be:

{"answer": "\\frac{1}{8}\\left( \\ln\\left(\\frac{5}{3}\\right) - \\frac{2}{5} \\right)", "numerical_answer": "0.01385320297"}

Let me check the numerical approximation again. Using a calculator, compute (ln(5/3) - 0.4)/8.

ln(5/3) ≈ 0.5108256237669907

0.5108256237669907 - 0.4 = 0.1108256237669907

0.1108256237669907 / 8 = 0.013853202970873837

Rounded to 10 decimal places: 0.01385320297. Yes, that's correct.
</think>

{"answer": "\\frac{1}{8}\\left( \\ln\\left(\\frac{5}{3}\\right) - \\frac{2}{5} \\right)", "numerical_answer": "0.01385320297"}