
To solve the definite integral \(\int_{0}^{7}\left(\sqrt[3]{\sqrt{x^{2}+1}+x}-\sqrt[3]{\sqrt{x^{2}+1}-x}\right)\,\mathrm{d}x\), we proceed as follows:


### Step 1: Simplify the Integrand
Let \( A = \sqrt[3]{\sqrt{x^2 + 1} + x} \) and \( B = \sqrt[3]{\sqrt{x^2 + 1} - x} \). The integrand is \( A - B \). 

First, note that:
\[
A^3 = \sqrt{x^2 + 1} + x \quad \text{and} \quad B^3 = \sqrt{x^2 + 1} - x.
\]
Multiplying \( A \) and \( B \):
\[
AB = \sqrt[3]{(\sqrt{x^2 + 1} + x)(\sqrt{x^2 + 1} - x)} = \sqrt[3]{(x^2 + 1) - x^2} = \sqrt[3]{1} = 1.
\]
Thus, \( B = \frac{1}{A} \), so the integrand simplifies to \( A - \frac{1}{A} \).


### Step 2: Substitution
Let \( t = A \), so \( t = \sqrt[3]{\sqrt{x^2 + 1} + x} \). Then \( t^3 = \sqrt{x^2 + 1} + x \). Solving for \( x \):
\[
t^3 - x = \sqrt{x^2 + 1}.
\]
Squaring both sides:
\[
(t^3 - x)^2 = x^2 + 1 \implies t^6 - 2t^3x + x^2 = x^2 + 1 \implies x = \frac{t^6 - 1}{2t^3} = \frac{t^3}{2} - \frac{1}{2t^3}.
\]
Differentiating \( x \) with respect to \( t \):
\[
\frac{dx}{dt} = \frac{3t^2}{2} + \frac{3}{2t^4} = \frac{3}{2}\left(t^2 + \frac{1}{t^4}\right).
\]


### Step 3: Rewrite the Integral
The integrand \( A - \frac{1}{A} \) becomes \( t - \frac{1}{t} \). The integral transforms to:
\[
\int_{t=1}^{t=T} \left(t - \frac{1}{t}\right) \cdot \frac{3}{2}\left(t^2 + \frac{1}{t^4}\right) dt,
\]
where \( T \) is the value of \( t \) when \( x = 7 \). Expanding the integrand:
\[
\left(t - \frac{1}{t}\right)\left(t^2 + \frac{1}{t^4}\right) = t^3 + \frac{1}{t^3} - t - \frac{1}{t^5}.
\]
Integrating term-by-term:
\[
\int \left(t^3 + \frac{1}{t^3} - t - \frac{1}{t^5}\right) dt = \frac{t^4}{4} - \frac{1}{2t^2} - \frac{t^2}{2} + \frac{1}{4t^4} + C.
\]


### Step 4: Evaluate the Definite Integral
The limits of integration for \( t \) are:
- When \( x = 0 \), \( t^3 = \sqrt{0 + 1} + 0 = 1 \implies t = 1 \).
- When \( x = 7 \), \( t^3 = \sqrt{7^2 + 1} + 7 = 7 + 5\sqrt{2} \). Let \( T = \sqrt[3]{7 + 5\sqrt{2}} \).

Evaluating the antiderivative at \( t = T \) and \( t = 1 \):
- At \( t = 1 \):
  \[
  \frac{1^4}{4} - \frac{1}{2 \cdot 1^2} - \frac{1^2}{2} + \frac{1}{4 \cdot 1^4} = \frac{1}{4} - \frac{1}{2} - \frac{1}{2} + \frac{1}{4} = -\frac{1}{2}.
  \]
- At \( t = T \): Using \( T - \frac{1}{T} = 2 \) (derived from \( T^3 - \frac{1}{T^3} = 14 \)), we find \( T^2 + \frac{1}{T^2} = 6 \) and \( T^4 + \frac{1}{T^4} = 34 \). Substituting:
  \[
  \frac{T^4}{4} - \frac{1}{2T^2} - \frac{T^2}{2} + \frac{1}{4T^4} = \frac{34}{4} - \frac{6}{2} = \frac{17}{2} - 3 = \frac{11}{2}.
  \]

Thus, the definite integral is:
\[
\frac{3}{2} \left( \frac{11}{2} - \left(-\frac{1}{2}\right) \right) = \frac{3}{2} \cdot 6 = 9.
\]


### Numerical Approximation
The exact value is \( 9 \), so the numerical approximation is \( 9.0000000000 \).


{"answer": "9", "numerical_answer": "9.0000000000"}