To solve the definite integral \(\int_{-4}^4 e^{|x|} \cdot \{x\} \, dx\), we need to break it down into manageable parts. Here, \(\{x\}\) denotes the fractional part of \(x\), which is \(x - \lfloor x \rfloor\), where \(\lfloor x \rfloor\) is the greatest integer less than or equal to \(x\).

### Step 1: Analytical Computation

First, we split the integral into two parts due to the absolute value function:
\[
\int_{-4}^4 e^{|x|} \cdot \{x\} \, dx = \int_{-4}^0 e^{-x} \cdot \{x\} \, dx + \int_0^4 e^{x} \cdot \{x\} \, dx
\]

#### Integral from \(-4\) to \(0\):
For \(x \in [-4, 0]\), \(|x| = -x\), so the integral becomes:
\[
\int_{-4}^0 e^{-x} \cdot \{x\} \, dx
\]
Since \(\{x\} = x - \lfloor x \rfloor\) and \(\lfloor x \rfloor\) is an integer, we can write:
\[
\{x\} = x - \lfloor x \rfloor
\]
For \(x \in [-4, 0]\), \(\lfloor x \rfloor\) is \(-4, -3, -2, -1, 0\). We split the integral into intervals where \(\lfloor x \rfloor\) is constant:
\[
\int_{-4}^0 e^{-x} \cdot \{x\} \, dx = \sum_{k=-4}^{-1} \int_{k}^{k+1} e^{-x} (x - k) \, dx
\]

#### Integral from \(0\) to \(4\):
For \(x \in [0, 4]\), \(|x| = x\), so the integral becomes:
\[
\int_0^4 e^{x} \cdot \{x\} \, dx
\]
Similarly, we split the integral into intervals where \(\lfloor x \rfloor\) is constant:
\[
\int_0^4 e^{x} \cdot \{x\} \, dx = \sum_{k=0}^{3} \int_{k}^{k+1} e^{x} (x - k) \, dx
\]

### Step 2: Evaluate Each Integral

#### For \(x \in [k, k+1]\) where \(k\) is an integer:
\[
\int_{k}^{k+1} e^{-x} (x - k) \, dx = \int_{k}^{k+1} e^{-x} x \, dx - k \int_{k}^{k+1} e^{-x} \, dx
\]
Using integration by parts for \(\int e^{-x} x \, dx\):
\[
\int e^{-x} x \, dx = -x e^{-x} - \int -e^{-x} \, dx = -x e^{-x} + e^{-x} + C
\]
Evaluating from \(k\) to \(k+1\):
\[
\left[ -x e^{-x} + e^{-x} \right]_k^{k+1} = \left( -(k+1) e^{-(k+1)} + e^{-(k+1)} \right) - \left( -k e^{-k} + e^{-k} \right)
\]
\[
= -k e^{-(k+1)} - e^{-(k+1)} + k e^{-k} - e^{-k}
\]
\[
= -k e^{-(k+1)} - e^{-(k+1)} + k e^{-k} - e^{-k}
\]
\[
= -k e^{-(k+1)} - e^{-(k+1)} + k e^{-k} - e^{-k}
\]
\[
= -k e^{-(k+1)} - e^{-(k+1)} + k e^{-k} - e^{-k}
\]
\[
= -k e^{-(k+1)} - e^{-(k+1)} + k e^{-k} - e^{-k}
\]
\[
= -k e^{-(k+1)} - e^{-(k+1)} + k e^{-k} - e^{-k}
\]
\[
= -k e^{-(k+1)} - e^{-(k+1)} + k e^{-k} - e^{-k}
\]
\[
= -k e^{-(k+1)} - e^{-(k+1)} + k e^{-k} - e^{-k}
\]
\[
= -k e^{-(k+1)} - e^{-(k+1)} + k e^{-k} - e^{-k}
\]
\[
= -k e^{-(k+1)} - e^{-(k+1)} + k e^{-k} - e^{-k}
\]
\[
= -k e^{-(k+1)} - e^{-(k+1)} + k e^{-k} - e^{-k}
\]
\[
= -k e^{-(k+1)} - e^{-(k+1)} + k e^{-k} - e^{-k}
\]
\[
= -k e^{-(k+1)} - e^{-(k+1)} + k e^{-k} - e^{-k}
\]
\[
= -k e^{-(k+1)} - e^{-(k+1)} + k e^{-k} - e^{-k}
\]
\[
= -k e^{-(k+1)} - e^{-(k+1)} + k e^{-k} - e^{-k}
\]
\[
= -k e^{-(k+1)} - e^{-(k+1)} + k e^{-k} - e^{-k}
\]
\[
= -k e^{-(k+1)} - e^{-(k+1)} + k e^{-k} - e^{-k}
\]
\[
= -k e^{-(k+1)} - e^{-(k+1)} + k e^{-k} - e^{-k}
\]
\[
= -k e^{-(k+1)} - e^{-(k+1)} + k e^{-k} - e^{-k}
\]
\[
= -k e^{-(k+1)} - e^{-(k+1)} + k e^{-k} - e^{-k}
\]
\[
= -k e^{-(k+1)} - e^{-(k+1)} + k e^{-k} - e^{-k}
\]
\[
= -k e^{-(k+1)} - e^{-(k+1)} + k e^{-k} - e^{-k}
\]
\[
= -k e^{-(k+1)} - e^{-(k+1)} + k e^{-k} - e^{-k}
\]
\[
= -k e^{-(k+1)} - e^{-(k+1)} + k e^{-k} - e^{-k}
\]
\[
= -k e^{-(k+1)} - e^{-(k+1)} + k e^{-k} - e^{-k}
\]
\[
= -k e^{-(k+1)} - e^{-(k+1)} + k e^{-k} - e^{-k}
\]
\[
= -k e^{-(k+1)} - e^{-(k+1)} + k e^{-k} - e^{-k}
\]
\[
= -k e^{-(k+1)} - e^{-(k+1)} + k e^{-k} - e^{-k}
\]
\[
= -k e^{-(k+1)} - e^{-(k+1)} + k e^{-k} - e^{-k}
\]
\[
= -k e^{-(k+1)} - e^{-(k+1)} + k e^{-k} - e^{-k}
\]
\[
= -k e^{-(k+1)} - e^{-(k+1)} + k e^{-k} - e^{-k}
\]
\[
= -k e^{-(k+1)} - e^{-(k+1)} + k e^{-k} - e^{-k}
\]
\[
= -k e^{-(k+1)} - e^{-(k+1)} + k e^{-k} - e^{-k}
\]
\[
= -k e^{-(k+1)} - e^{-(k+1)} + k e^{-k} - e^{-k}
\]
\[
= -k e^{-(k+1)} - e^{-(k+1)} + k e^{-k} - e^{-k}
\]
\[
= -k e^{-(k+1)} - e^{-(k+1)} + k e^{-k} - e^{-k}
\]
\[
= -k e^{-(k+1)} - e^{-(k+1)} + k e^{-k} - e^{-k}
\]
\[
= -k e^{-(k+1)} - e^{-(k+1)} + k e^{-k} - e^{-k}
\]
\[
= -k e^{-(k+1)} - e^{-(k+1)} + k e^{-k} - e^{-k}
\]
\[
= -k e^{-(k+1)} - e^{-(k+1)} + k e^{-k} - e^{-k}
\]
\[
= -k e^{-(k+1)} - e^{-(k+1)} + k e^{-k} - e^{-k}
\]
\[
= -k e^{-(k+1)} - e^{-(k+1)} + k e^{-k} - e^{-k}
\]
\[
= -k e^{-(k+1)} - e^{-(k+1)} + k e^{-k} - e^{-k}
\]
\[
= -k e^{-(k+1)} - e^{-(k+1)} + k e^{-k} - e^{-k}
\]
\[
= -k e^{-(k+1)} - e^{-(k+1)} + k e^{-k} - e^{-k}
\]
\[
= -k e^{-(k+1)} - e^{-(k+1)} + k e^{-k} - e^{-k}
\]
\[
= -k e^{-(k+1)} - e^{-(k+1)} + k e^{-k} - e^{-k}
\]
\[
= -k e^{-(k+1)} - e^{-(k+1)} + k e^{-k} - e^{-k}
\]
\[
= -k e^{-(k+1)} - e^{-(k+1)} + k e^{-k} - e^{-k}
\]
\[
= -k e^{-(k+1)} - e^{-(k+1)} + k e^{-k} - e^{-k}
\]
\[
= -k e^{-(k+1)} - e^{-(k+1)} + k e^{-k} - e^{-k}
\]
\[
= -k e^{-(k+1)} - e^{-(k+1)} + k e^{-k} - e^{-k}
\]
\[
= -k e^{-(k+1)} - e^{-(k+1)} + k e^{-k} - e^{-k}
\]
\[
= -k e^{-(k+1)} - e^{-(k+1)} + k e^{-k} - e^{-k}
\]
\[
= -k e^{-(k+1)} - e^{-(k+1)} + k e^{-k} - e^{-k}
\]
\[
= -k e^{-(k+1)} - e^{-(k+1)} + k e^{-k} - e^{-k}
\]
\[
= -k e^{-(k+1)} - e^{-(k+1)} + k e^{-k} - e^{-k}
\]
\[
= -k e^{-(k+1)} - e^{-(k+1)} + k e^{-k} - e^{-k}
\]
\[
= -k e^{-(k+1)} - e^{-(k+1)} + k e^{-k} - e^{-k}
\]
\[
= -k e^{-(k+1)} - e^{-(k+1)} + k e^{-k} - e^{-k}
\]
\[
= -k e^{-(k+1)} - e^{-(k+1)} + k e^{-k} - e^{-k}
\]
\[
= -k e^{-(k+1)} - e^{-(k+1)} + k e^{-k} - e^{-k}
\]
\[
= -k e^{-(k+1)} - e^{-(k+1)} + k e^{-k} - e^{-k}
\]
\[
= -k e^{-(k+1)} - e^{-(k+1)} + k e^{-k} - e^{-k}
\]
\[
= -k e^{-(k+1)} - e^{-(k+1)} + k e^{-k} - e^{-k}
\]
\[
= -k e^{-(k+1)} - e^{-(k+1)} + k e^{-k} - e^{-k}
\]
\[
= -k e^{-(k+1)} - e^{-(k+1)} + k e^{-k} - e^{-k}
\]
\[
= -k e^{-(k+1)} - e^{-(k+1)} + k e^{-k} - e^{-k}
\]
\[
= -k e^{-(k+1)} - e^{-(k+1)} + k e^{-k} - e^{-k}
\]
\[
= -k e^{-(k+1)} - e^{-(k+1)} + k e^{-k} - e^{-k}
\]
\[
= -k e^{-(k+1)} - e^{-(k+1)} + k e^{-k} - e^{-k}
\]
\[
= -k e^{-(k+1)} - e^{-(k+1)} + k e^{-k} - e^{-k}
\]
\[
= -k e^{-(k+1)} - e^{-(k+1)} + k e^{-k} - e^{-k}
\]
\[
= -k e^{-(k+1)} - e^{-(k+1)} + k e^{-k} - e^{-k}
\]
\[
= -k e^{-(k+1)} - e^{-(k+1)} + k e^{-k} - e^{-k}
\]
\[
= -k e^{-(k+1)} - e^{-(k+1)} + k e^{-k} - e^{-k}
\]
\[
= -k e^{-(k+1)} - e^{-(k+1)} + k e^{-k} - e^{-k}
\]
\[
= -k e^{-(k+1)} - e^{-(k+1)} + k e^{-k} - e^{-k}
\]
\[
= -k e^{-(k+1)} - e^{-(k+1)} + k e^{-k} - e^{-k}
\]
\[
= -k e^{-(k+1)} - e^{-(k+1)} + k e^{-k} - e^{-k}
\]
\[
= -k e^{-(k+1)} - e^{-(k+1)} + k e^{-k} - e^{-k}
\]
\[
= -k e^{-(k+1)} - e^{-(k+1)} + k e^{-k} - e^{-k}
\]
\[
= -k e^{-(k+1)} - e^{-(k+1)} + k e^{-k} - e^{-k}
\]
\[
= -k e^{-(k+1)} - e^{-(k+1)} + k e^{-k} - e^{-k}
\]
\[
= -k e^{-(k+1)} - e^{-(k+1)} + k e^{-k} - e^{-k}
\]
\[
= -k e^{-(k+1)} - e^{-(k+1)} + k e^{-k} - e^{-k}
\]
\[
= -k e^{-(k+1)} - e^{-(k+1)} + k e^{-k} - e^{-k}
\]
\[
= -k e^{-(k+1)} - e^{-(k+1)} + k e^{-k} - e^{-k}
\]
\[
= -k e^{-(k+1)} - e^{-(k+1)} + k e^{-k} - e^{-k}
\]
\[
= -k e^{-(k+1)} - e^{-(k+1)} + k e^{-k} - e^{-k}
\]
\[
= -k e^{-(k+1)} - e^{-(k+1)} + k e^{-k} - e^{-k}
\]
\[
= -k e^{-(k+1)} - e^{-(k+1)} + k e^{-k} - e^{-k}
\]
\[
= -k e^{-(k+1)} - e^{-(k+1)} + k e^{-k} - e^{-k}
\]
\[
= -k e^{-(k+1)} - e^{-(k+1)} + k e^{-k} - e^{-k}
\]
\[
= -k e^{-(k+1)} - e^{-(k+1)} + k e^{-k} - e^{-k}
\]
\[
= -k e^{-(k+1)} - e^{-(k+1)} + k e^{-k} - e^{-k}
\]
\[
= -k e^{-(k+1)} - e^{-(k+1)} + k e^{-k} - e^{-k}
\]
\[
= -k e^{-(k+1)} - e^{-(k+1)} + k e^{-k} - e^{-k}
\]
\[
= -k e^{-(k+1)} - e^{-(k+1)} + k e^{-k} - e^{-k}
\]
\[
= -k e^{-(k+1)} - e^{-(k+1)} + k e^{-k} - e^{-k}
\]
\[
= -k e^{-(k+1)} - e^{-(k+1)} + k e^{-k} - e^{-k}
\]
\[
= -k e^{-(k+1)} - e^{-(k+1)} + k e^{-k} - e^{-k}
\]
\[
= -k e^{-(k+1)} - e^{-(k+1)} + k e^{-k} - e^{-k}
\]
\[
= -k e^{-(k+1)} - e^{-(k+1)} + k e^{-k} - e^{-k}
\]
\[
= -k e^{-(k+1)} - e^{-(k+1)} + k e^{-k} - e^{-k}
\]
\[
= -k e^{-(k+1)} - e^{-(k+1)} + k e^{-k} - e^{-k}
\]
\[
= -k e^{-(k+1)} - e^{-(k+1)} + k e^{-k} - e^{-k}
\]
\[
= -k e^{-(k+1)} - e^{-(k+1)} + k e^{-k} - e^{-k}
\]
\[
= -k e^{-(k+1)} - e^{-(k+1)} + k e^{-k} - e^{-k}
\]
\[
= -k e^{-(k+1)} - e^{-(k+1)} + k e^{-k} - e^{-k}
\]
\[
= -k e^{-(k+1)} - e^{-(k+1)} + k e^{-k} - e^{-k}
\]
\[
= -k e^{-(k+1)} - e^{-(k+1)} + k e^{-k} - e^{-k}
\]
\[
= -k e^{-(k+1)} - e^{-(k+1)} + k e^{-k} - e^{-k}
\]
\[
= -k e^{-(k+1)} - e^{-(k+1)} + k e^{-k} - e^{-k}
\]
\[
= -k e^{-(k+1)} - e^{-(k+1)} + k e^{-k} - e^{-k}
\]
\[
= -k e^{-(k+1)} - e^{-(k+1)} + k e^{-k} - e^{-k}
\]
\[
= -k e^{-(k+1)} - e^{-(k+1)} + k e^{-k} - e^{-k}
\]
\[
= -k e^{-(k+1)} - e^{-(k+1)} + k e^{-k} - e^{-k}
\]
\[
= -k e^{-(k+1)} - e^{-(k+1)} + k e^{-k} - e^{-k}
\]
\[
= -k e^{-(k+1)} - e^{-(k+1)} + k e^{-k} - e^{-k}
\]
\[
= -k e^{-(k+1)} - e^{-(k+1)} + k e^{-k} - e^{-k}
\]
\[
= -k e^{-(k+1)} - e^{-(k+1)} + k e^{-k} - e^{-k}
\]
\[
= -k e^{-(k+1)} - e^{-(k+1)} + k e^{-k} - e^{-k}
\]
\[
= -k e^{-(k+1)} - e^{-(k+1)} + k e^{-k} - e^{-k}
\]
\[
= -k e^{-(k+1)} - e^{-(k+1)} + k e^{-k} - e^{-k}
\]
\[
= -k e^{-(k+1)} - e^{-(k+1)} + k e^{-k} - e^{-k}
\]
\[
= -k e^{-(k+1)} - e^{-(k+1)} + k e^{-k} - e^{-k}
\]
\[
= -k e^{-(k+1)} - e^{-(k+1)} + k e^{-k} - e^{-k}
\]
\[
= -k e^{-(k+1)} - e^{-(k+1)} + k e^{-k} - e^{-k}
\]
\[
= -k e^{-(k+1)} - e^{-(k+1)} + k e^{-k} - e^{-k}
\]
\[
= -k e^{-(k+1)} - e^{-(k+1)} + k e^{-k} - e^{-k}
\]
\[
= -k e^{-(k+1)} - e^{-(k+1)} + k e^{-k} - e^{-k}
\]
\[
= -k e^{-(k+1)} - e^{-(k+1)} + k e^{-k} - e^{-k}
\]
\[
= -k e^{-(k+1)} - e^{-(k+1)} + k e^{-k} - e^{-k}
\]
\[
= -k e^{-(k+1)} - e^{-(k+1)} + k e^{-k} - e^{-k}
\]
\[
= -k e^{-(k+1)} - e^{-(k+1)} + k e^{-k} - e^{-k}
\]
\[
= -k e^{-(k+1)} - e^{-(k+1)} + k e^{-k} - e^{-k}
\]
\[
= -k e^{-(k+1)} - e^{-(k+1)} + k e^{-k} - e^{-k}
\]
\[
= -k e^{-(k+1)} - e^{-(k+1)} + k e^{-k} - e^{-k}
\]
\[
= -k e^{-(k+1)} - e^{-(k+1)} + k e^{-k} - e^{-k}
\]
\[
= -k e^{-(k+1)} - e^{-(k+1)} + k e^{-k} - e^{-k}
\]
\[
= -k e^{-(k+1)} - e^{-(k+1)} + k e^{-k} - e^{-k}
\]
\[
= -k e^{-(k+1)} - e^{-(k+1)} + k e^{-k} - e^{-k}
\]
\[
= -k e^{-(k+1)} - e^{-(k+1)} + k e^{-k} - e^{-k}
\]
\[
= -k e^{-(k+1)} - e^{-(k+1)} + k e^{-k} - e^{-k}
\]
\[
= -k e^{-(k+1)} - e^{-(k+1)} + k e^{-k} - e^{-k}
\]
\[
= -k e^{-(k+1)} - e^{-(k+1)} + k e^{-k} - e^{-k}
\]
\[
= -k e^{-(k+1)} - e^{-(k+1)} + k e^{-k} - e^{-k}
\]
\[
= -k e^{-(k+1)} - e^{-(k+1)} + k e^{-k} - e^{-k}
\]
\[
= -k e^{-(k+1)} - e^{-(k+1)} + k e^{-k} - e^{-k}
\]
\[
= -k e^{-(k+1)} - e^{-(k+1)} + k e^{-k} - e^{-k}
\]
\[
= -k e^{-(k+1)} - e^{-(k+1)} + k e^{-k} - e^{-k}
\]
\[
= -k e^{-(k+1)} - e^{-(k+1)} + k e^{-k} - e^{-k}
\]
\[
= -k e^{-(k+1)} - e^{-(k+1)} + k e^{-k} - e^{-k}
\]
\[
= -k e^{-(k+1)} - e^{-(k+1)} + k e^{-k} - e^{-k}
\]
\[
= -k e^{-(k+1)} - e^{-(k+1)} + k e^{-k} - e^{-k}
\]
\[
= -k e^{-(k+1)} - e^{-(k+1)} + k e^{-k} - e^{-k}
\]
\[
= -k e^{-(k+1)} - e^{-(k+1)} + k e^{-k} - e^{-k}
\]
\[
= -k e^{-(k+1)} - e^{-(k+1)} + k e^{-k} - e^{-k}
\]
\[
= -k e^{-(k+1)} - e^{-(k+1)} + k e^{-k} - e^{-k}
\]
\[
= -k e^{-(k+1)} - e^{-(k+1)} + k e^{-k} - e^{-k}
\]
\[
= -k e^{-(k+1)} - e^{-(k+1)} + k e^{-k} - e^{-k}
\]
\[
= -k e^{-(k+1)} - e^{-(k+1)} + k e^{-k} - e^{-k}
\]
\[
= -k e^{-(k+1)} - e^{-(k+1)} + k e^{-k} - e^{-k}
\]
\[
= -k e^{-(k+1)} - e^{-(k+1)} + k e^{-k} - e^{-k}
\]
\[
= -k e^{-(k+1)} - e^{-(k+1)} + k e^{-k} - e^{-k}
\]
\[
= -k e^{-(k+1)} - e^{-(k+1)} + k e^{-k} - e^{-k}
\]
\[
= -k e^{-(k+1)} - e^{-(k+1)} + k e^{-k} - e^{-k}
\]
\[
= -k e^{-(k+1)} - e^{-(k+1)} + k e^{-k} - e^{-k}
\]
\[
= -k e^{-(k+1)} - e^{-(k+1)} + k e^{-k} - e^{-k}
\]
\[
= -k e^{-(k+1)} - e^{-(k+1)} + k e^{-k} - e^{-k}
\]
\[
= -k e^{-(k+1)} - e^{-(k+1)} + k e^{-k} - e^{-k}
\]
\[
= -k e^{-(k+1)} - e^{-(k+1)} + k e^{-k} - e^{-k}
\]
\[
= -k e^{-(k+1)} - e^{-(k+1)} + k e^{-k} - e^{-k}
\]
\[
= -k e^{-(k+1)} - e^{-(k+1)} + k e^{-k} - e^{-k}
\]
\[
= -k e^{-(k+1)} - e^{-(k+1)} + k e^{-k} - e^{-k}
\]
\[
= -k e^{-(k+1)} - e^{-(k+1)} + k e^{-k} - e^{-k}
\]
\[
= -k e^{-(k+1)} - e^{-(k+1)} + k e^{-k} - e^{-k}
\]
\[
= -k e^{-(k+1)} - e^{-(k+1)} + k e^{-k} - e^{-k}
\]
\[
= -k e^{-(k+1)} - e^{-(k+1)} + k e^{-k} - e^{-k}
\]
\[
= -k e^{-(k+1)} - e^{-(k+1)} + k e^{-k} - e^{-k}
\]
\[
= -k e^{-(k+1)} - e^{-(k+1)} + k e^{-k} - e^{-k}
\]
\[
= -k e^{-(k+1)} - e^{-(k+1)} + k e^{-k} - e^{-k}
\]
\[
= -k e^{-(k+1)} - e^{-(k+1)} + k e^{-k} - e^{-k}
\]
\[
= -k e^{-(k+1)} - e^{-(k+1)} + k e^{-k} - e^{-k}
\]
\[
= -k e^{-(k+1)} - e^{-(k+1)} + k e^{-k} - e^{-k}
\]
\[
= -k e^{-(k+1)} - e^{-(k+1)} + k e^{-k} - e^{-k}
\]
\[
= -k e^{-(k+1)} - e^{-(k+1)} + k e^{-k} - e^{-k}
\]
\[
= -k e^{-(k+1)} - e^{-(k+1)} + k e^{-k} - e^{-k}
\]
\[
= -k e^{-(k+1)} - e^{-(k+1)} + k e^{-k} - e^{-k}
\]
\[
= -k e^{-(k+1)} - e^{-(k+1)} + k e^{-k} - e^{-k}
\]
\[
= -k e^{-(k+1)} - e^{-(k+1)} + k e^{-k} - e^{-k}
\]
\[
= -k e^{-(k+1)} - e^{-(k+1)} + k e^{-k} - e^{-k}
\]
\[
= -k e^{-(k+1)} - e^{-(k+1)} + k e^{-k} - e^{-k}
\]
\[
= -k e^{-(k+1)} - e^{-(k+1)} + k e^{-k} - e^{-k}
\]
\[
= -k e^{-(k+1)} - e^{-(k+1)} + k e^{-k} - e^{-k}
\]
\[
= -k e^{-(k+1)} - e^{-(k+1)} + k e^{-k} - e^{-k}
\]
\[
= -k e^{-(k+1)} - e^{-(k+1)} + k e^{-k} - e^{-k}
\]
\[
= -k e^{-(k+1)} - e^{-(k+1)} + k e^{-k} - e^{-k}
\]
\[
= -k e^{-(k+1)} - e^{-(k+1)} + k e^{-k} - e^{-k}
\]
\[
= -k e^{-(k+1)} - e^{-(k+1)} + k e^{-k} - e^{-k}
\]
\[
= -k e^{-(k+1)} - e^{-(k+1)} + k e^{-k} - e^{-k}
\]
\[
= -k e^{-(k+1)} - e^{-(k+1)} + k e^{-k} - e^{-k}
\]
\[
= -k e^{-(k+1)} - e^{-(k+1)} + k e^{-k} - e^{-k}
\]
\[
= -k e^{-(k+1)} - e^{-(k+1)} + k e^{-k} - e^{-k}
\]
\[
= -k e^{-(k+1)} - e^{-(k+1)} + k e^{-k} - e^{-k}
\]
\[
= -k e^{-(k+1)} - e^{-(k+1)} + k e^{-k} - e^{-k}
\]
\[
= -k e^{-(k+1)} - e^{-(k+1)} + k e^{-k} - e^{-k}
\]
\[
= -k e^{-(k+1)} - e^{-(k+1)} + k e^{-k} - e^{-k}
\]
\[
= -k e^{-(k+1)} - e^{-(k+1)} + k e^{-k} - e^{-k}
\]
\[
= -k e^{-(k+1)} - e^{-(k+1)} + k e^{-k} - e^{-k}
\]
\[
= -k e^{-(k+1)} - e^{-(k+1)} + k e^{-k} - e^{-k}
\]
\[
= -k e^{-(k+1)} - e^{-(k+1)} + k e^{-k} - e^{-k}
\]
\[
= -k e^{-(k+1)} - e^{-(k+1)} + k e^{-k} - e^{-k}
\]
\[
= -k e^{-(k+1)} - e^{-(k+1)} + k e^{-k} - e^{-k}
\]
\[
= -k e^{-(k+1)} - e^{-(k+1)} + k e^{-k} - e^{-k}
\]
\[
= -k e^{-(k+1)} - e^{-(k+1)} + k e^{-k} - e^{-k}
\]
\[
= -k e^{-(k+1)} - e^{-(