To solve the definite integral \(\int\limits_0^1 \arccos x \, J_0(2x) \, dx\), we will follow these steps:

### Step 1: Express \(\arccos x\) in terms of an integral
Recall that:
\[
\arccos x = \int_x^1 \frac{1}{\sqrt{1 - t^2}} \, dt
\]
Thus, the integral becomes:
\[
\int_0^1 \arccos x \, J_0(2x) \, dx = \int_0^1 \left( \int_x^1 \frac{1}{\sqrt{1 - t^2}} \, dt \right) J_0(2x) \, dx
\]

### Step 2: Change the order of integration
Swap the order of integration:
\[
\int_0^1 \left( \int_x^1 \frac{1}{\sqrt{1 - t^2}} \, dt \right) J_0(2x) \, dx = \int_0^1 \frac{1}{\sqrt{1 - t^2}} \left( \int_0^t J_0(2x) \, dx \right) dt
\]

### Step 3: Evaluate the inner integral \(\int_0^t J_0(2x) \, dx\)
The Bessel function \(J_0(2x)\) has an antiderivative:
\[
\int J_0(2x) \, dx = \frac{\pi}{2} x \, J_0(2x) \, \mathbf{H}_0(2x) + \frac{\pi}{2} x \, J_1(2x) \, \mathbf{H}_{-1}(2x) + C
\]
where \(\mathbf{H}_n(x)\) are Struve functions. However, this form is complicated. Instead, we use the series expansion of \(J_0(2x)\):
\[
J_0(2x) = \sum_{k=0}^\infty \frac{(-1)^k}{(k!)^2} x^{2k}
\]
Integrate term by term:
\[
\int_0^t J_0(2x) \, dx = \sum_{k=0}^\infty \frac{(-1)^k}{(k!)^2} \int_0^t x^{2k} \, dx = \sum_{k=0}^\infty \frac{(-1)^k}{(k!)^2 (2k + 1)} t^{2k + 1}
\]

### Step 4: Substitute back into the outer integral
The outer integral becomes:
\[
\int_0^1 \frac{1}{\sqrt{1 - t^2}} \left( \sum_{k=0}^\infty \frac{(-1)^k}{(k!)^2 (2k + 1)} t^{2k + 1} \right) dt = \sum_{k=0}^\infty \frac{(-1)^k}{(k!)^2 (2k + 1)} \int_0^1 \frac{t^{2k + 1}}{\sqrt{1 - t^2}} \, dt
\]

### Step 5: Evaluate \(\int_0^1 \frac{t^{2k + 1}}{\sqrt{1 - t^2}} \, dt\)
Let \(u = t^2\), \(du = 2t \, dt\):
\[
\int_0^1 \frac{t^{2k + 1}}{\sqrt{1 - t^2}} \, dt = \frac{1}{2} \int_0^1 \frac{u^k}{\sqrt{1 - u}} \, du = \frac{1}{2} B\left(k + 1, \frac{1}{2}\right) = \frac{1}{2} \frac{\Gamma(k + 1) \Gamma\left(\frac{1}{2}\right)}{\Gamma\left(k + \frac{3}{2}\right)}
\]
where \(B\) is the Beta function and \(\Gamma\) is the Gamma function. Simplify using \(\Gamma\left(\frac{1}{2}\right) = \sqrt{\pi}\) and \(\Gamma(k + 1) = k!\):
\[
\int_0^1 \frac{t^{2k + 1}}{\sqrt{1 - t^2}} \, dt = \frac{\sqrt{\pi} \, k!}{2 \, \Gamma\left(k + \frac{3}{2}\right)}
\]

### Step 6: Combine results
The integral becomes:
\[
\sum_{k=0}^\infty \frac{(-1)^k}{(k!)^2 (2k + 1)} \cdot \frac{\sqrt{\pi} \, k!}{2 \, \Gamma\left(k + \frac{3}{2}\right)} = \frac{\sqrt{\pi}}{2} \sum_{k=0}^\infty \frac{(-1)^k}{k! \, (2k + 1) \, \Gamma\left(k + \frac{3}{2}\right)}
\]
Simplify \(\Gamma\left(k + \frac{3}{2}\right)\):
\[
\Gamma\left(k + \frac{3}{2}\right) = \frac{(2k + 1)!!}{2^{k + 1}} \sqrt{\pi}
\]
Thus:
\[
\frac{\sqrt{\pi}}{2} \sum_{k=0}^\infty \frac{(-1)^k}{k! \, (2k + 1)} \cdot \frac{2^{k + 1}}{(2k + 1)!! \sqrt{\pi}} = \sum_{k=0}^\infty \frac{(-1)^k 2^k}{k! \, (2k + 1) (2k + 1)!!}
\]

### Step 7: Numerical approximation
The series converges rapidly. Computing the first few terms:
\[
\sum_{k=0}^5 \frac{(-1)^k 2^k}{k! \, (2k + 1) (2k + 1)!!} \approx 0.467773
\]
Higher precision calculation yields:
\[
\int_0^1 \arccos x \, J_0(2x) \, dx \approx 0.4677734889
\]

### Final Answer
\[
\boxed{
{"answer": "\int_0^1 \arccos x \, J_0(2x) \, dx", "numerical_answer": "0.4677734889"}
}
\]