
To solve the definite integral \(\int_{0}^{1} x^{-3/4}(1-x)^{-1/4}\left[1 - \sqrt{x(1-x)}\right]^{-2} \, dx\), we proceed with the following steps:


### Step 1: Substitution to Simplify the Integrand
We use the substitution \( t = \frac{\sqrt{x}}{\sqrt{1-x}} \), which implies \( x = \frac{t^2}{1+t^2} \) and \( dx = \frac{2t}{(1+t^2)^2} \, dt \). This transforms the original integral into a more manageable form. 

Under this substitution:
- \( x^{-3/4} = \left(\frac{t^2}{1+t^2}\right)^{-3/4} = \frac{(1+t^2)^{3/4}}{t^{3/2}} \),
- \( (1-x)^{-1/4} = \left(\frac{1}{1+t^2}\right)^{-1/4} = (1+t^2)^{1/4} \),
- \( \sqrt{x(1-x)} = \frac{t}{1+t^2} \),
- The denominator \(\left[1 - \sqrt{x(1-x)}\right]^{-2} = \left(\frac{1+t^2 - t}{1+t^2}\right)^{-2} = \frac{(1+t^2)^2}{(t^2 - t + 1)^2}\).

Substituting these into the integral and simplifying, we find the integral reduces to:
\[
4 \int_{0}^{\infty} \frac{1 + u^4}{(u^4 - u^2 + 1)^2} \, du
\]
where \( u = \sqrt{t} \).


### Step 2: Evaluating the Transformed Integral
We split the integrand as \( \frac{1 + u^4}{(u^4 - u^2 + 1)^2} = \frac{1}{u^4 - u^2 + 1} + \frac{u^2}{(u^4 - u^2 + 1)^2} \). Let \( I = \int_{0}^{\infty} \frac{1}{u^4 - u^2 + 1} \, du \) and \( J = \int_{0}^{\infty} \frac{u^2}{(u^4 - u^2 + 1)^2} \, du \).

#### Evaluating \( I \):
Using the substitution \( v = u - \frac{1}{u} \), we find \( I = \frac{\pi}{2} \).

#### Evaluating \( J \):
By differentiating \( I \) with respect to a parameter \( a \) (where \( I(a) = \int_{0}^{\infty} \frac{1}{u^4 - a u^2 + 1} \, du \)), we find \( J = \frac{\pi}{4} \).


### Step 3: Combining Results
The original integral becomes \( 4(I + J) = 4\left(\frac{\pi}{2} + \frac{\pi}{4}\right) = 3\pi \).


### Numerical Approximation
The numerical value of \( 3\pi \) is approximately \( 9.4247779608 \).


{"answer": "3\\pi", "numerical_answer": "9.4247779608"}