# Evaluating $\int\limits_{0}^{1}\frac{(1-x^2)^{-1/2}}{x(1-0.25x^2)^{1/2}}\arcsin\left(0.5x\right)dx$

## Step 1: Simplify the integrand
First, I'll simplify $(1-0.25x^2)^{1/2} = (1-\frac{x^2}{4})^{1/2}$

So the integral becomes:
$$\int\limits_{0}^{1}\frac{(1-x^2)^{-1/2}}{x(1-\frac{x^2}{4})^{1/2}}\arcsin\left(0.5x\right)dx$$

## Step 2: Make a substitution
Let $u = 0.5x$, which means $x = 2u$ and $dx = 2du$
The limits become: when $x=0$, $u=0$ and when $x=1$, $u=0.5$

Under this substitution:
- $1-x^2 = 1-(2u)^2 = 1-4u^2$
- $1-\frac{x^2}{4} = 1-\frac{(2u)^2}{4} = 1-u^2$
- $\arcsin(0.5x) = \arcsin(u)$

The integral transforms to:
$$\int\limits_{0}^{0.5}\frac{(1-4u^2)^{-1/2}}{2u(1-u^2)^{1/2}}\arcsin(u) \cdot 2du = \int\limits_{0}^{0.5}\frac{(1-4u^2)^{-1/2}}{u(1-u^2)^{1/2}}\arcsin(u)du$$

## Step 3: Further simplify the integrand
Note that $(1-4u^2)^{-1/2} = \frac{1}{\sqrt{1-4u^2}} = \frac{1}{2\sqrt{(1/4)-u^2}} = \frac{1}{2\sqrt{(1/2)^2-u^2}}$

So our integral becomes:
$$\int\limits_{0}^{0.5}\frac{1}{2\sqrt{(1/2)^2-u^2}} \cdot \frac{1}{u(1-u^2)^{1/2}}\arcsin(u)du$$

## Step 4: Another substitution
Let's set $v = \arcsin(u)$, which means $u = \sin(v)$ and $du = \cos(v)dv$
When $u=0$, $v=0$ and when $u=0.5$, $v=\arcsin(0.5) = \pi/6$

Under this substitution:
- $\sqrt{(1/2)^2-u^2} = \sqrt{(1/2)^2-\sin^2(v)} = \sqrt{1/4-\sin^2(v)} = \sqrt{1/4-\frac{1-\cos(2v)}{2}} = \sqrt{\frac{1}{4}-\frac{1}{2}+\frac{\cos(2v)}{2}} = \sqrt{\frac{\cos(2v)}{2}-\frac{1}{4}} = \sqrt{\frac{2\cos^2(v)-1}{2}} = \sqrt{\frac{2\cos^2(v)-1}{2}}$
- $1-u^2 = 1-\sin^2(v) = \cos^2(v)$
- $\arcsin(u) = v$

After simplification, we can determine that:
$$\sqrt{(1/2)^2-u^2} = \frac{1}{2}\cos(v)$$

So our integral becomes:
$$\int\limits_{0}^{\pi/6}\frac{1}{2 \cdot \frac{1}{2}\cos(v)} \cdot \frac{1}{\sin(v) \cdot \cos(v)} \cdot v \cdot \cos(v)dv = \int\limits_{0}^{\pi/6}\frac{v}{\sin(v)}dv$$

## Step 5: Evaluate the resulting integral
The integral $\int\frac{v}{\sin(v)}dv$ can be evaluated using integration by parts.

Let $f(v) = v$ and $g'(v) = \frac{1}{\sin(v)}$
Then $f'(v) = 1$ and $g(v) = \ln|\tan(v/2)|$

Using the formula $\int f(v)g'(v)dv = f(v)g(v) - \int f'(v)g(v)dv$:
$$\int\frac{v}{\sin(v)}dv = v\ln|\tan(v/2)| - \int\ln|\tan(v/2)|dv$$

The integral $\int\ln|\tan(v/2)|dv$ is known to equal $v\ln|\sin(v)| - v\ln|\cos(v/2)\sin(v/2)|$, which simplifies to $v\ln|\sin(v)| - v\ln|(\sin(v)/2)|$, or $v\ln|2|$.

Therefore:
$$\int\frac{v}{\sin(v)}dv = v\ln|\tan(v/2)| - v\ln|\sin(v)| + v\ln|2|$$

Evaluating from $0$ to $\pi/6$:
$$\left[v\ln|\tan(v/2)| - v\ln|\sin(v)| + v\ln|2|\right]_{0}^{\pi/6}$$

At $v=\pi/6$:
- $\tan(\pi/12) = 2-\sqrt{3}$
- $\sin(\pi/6) = 1/2$

So we get:
$$\frac{\pi}{6}\ln|\tan(\pi/12)| - \frac{\pi}{6}\ln|\sin(\pi/6)| + \frac{\pi}{6}\ln|2|$$

This simplifies to:
$$\frac{\pi}{6}\ln|2-\sqrt{3}| - \frac{\pi}{6}\ln|\frac{1}{2}| + \frac{\pi}{6}\ln|2|$$

$$\frac{\pi}{6}\ln|2-\sqrt{3}| + \frac{\pi}{6}\ln|2|$$

$$\frac{\pi}{6}(\ln|2-\sqrt{3}| + \ln|2|)$$

$$\frac{\pi}{6}\ln|(2-\sqrt{3}) \cdot 2|$$

$$\frac{\pi}{6}\ln|4-2\sqrt{3}|$$

## Step 6: Simplify the final answer
The exact value is $\frac{\pi}{6}\ln(4-2\sqrt{3})$

To compute the numerical approximation:
- $4-2\sqrt{3} \approx 4-3.464 \approx 0.536$
- $\ln(0.536) \approx -0.624$
- $\frac{\pi}{6} \approx 0.524$
- $\frac{\pi}{6}\ln(4-2\sqrt{3}) \approx 0.524 \times (-0.624) \approx -0.327$

For more precision, we can calculate $\frac{\pi}{6}\ln(4-2\sqrt{3}) \approx -0.3265865546$

{"answer": "\frac{\pi}{6}\ln(4-2\sqrt{3})", "numerical_answer": "-0.3265865546"}