Given:

\[
I = \int_{0}^{2} x^{-1/2} (2-x)^{-1/2} \cos\left( \sqrt{x(2-x)} \right) dx
\]

Let’s proceed step by step.

### Step 1: Substitution

Set \( x = 2 \sin^2 \theta \), where \( 0 \leq \theta \leq \frac{\pi}{2} \).

- \( dx = 4 \sin\theta \cos\theta\, d\theta = 2 \sin(2\theta) d\theta \)
- \( x^{-1/2} = (2 \sin^2 \theta)^{-1/2} = (2)^{-1/2} \sin^{-1}\theta \)
- \( 2-x = 2(1 - \sin^2 \theta) = 2\cos^2\theta \implies (2-x)^{-1/2} = (2)^{-1/2} \cos^{-1}\theta \)
- \( \sqrt{x (2-x)} = \sqrt{2\sin^2\theta \cdot 2\cos^2\theta} = 2\sin\theta \cos\theta = \sin 2\theta \)

Plug in:

\[
I = \int_{\theta=0}^{\theta=\frac{\pi}{2}} 
(2)^{-1/2}\sin^{-1} \theta \cdot (2)^{-1/2}\cos^{-1} \theta \cos\left(\sin 2\theta\right) 2\sin 2\theta\, d\theta
\]

\[
= \frac{1}{2} \int_{0}^{\frac{\pi}{2}} \sin^{-1}\theta \cos^{-1}\theta \cos(\sin 2\theta) \sin 2\theta d\theta
\]

But note:
\[
\sin^{-1}\theta \cos^{-1}\theta = \frac{1}{\sin\theta \cos\theta}
\]
But that's not correct, because \(\sin^{-1}\theta = 1/\sin\theta\), \(\cos^{-1}\theta = 1/\cos\theta\), so their product is \(1/( \sin\theta \cos\theta)\).

But in the integrand, we had \(x^{-1/2} = (2 \sin^2\theta)^{-1/2} = (2)^{-1/2} \sin^{-1}\theta\), so it's as above.

Wait, go carefully:

\[
x^{-1/2} = (2 \sin^2\theta)^{-1/2} = \frac{1}{\sqrt{2}} \frac{1}{\sin\theta}
\]
\[
(2-x)^{-1/2} = (2 \cos^2\theta)^{-1/2} = \frac{1}{\sqrt{2}} \frac{1}{\cos\theta}
\]
So
\[
x^{-1/2}(2-x)^{-1/2} = \frac{1}{2} \frac{1}{\sin\theta \cos\theta}
\]

dx is:

\[
dx = 4\sin\theta \cos\theta d\theta = 2 \sin 2\theta d\theta
\]

So putting everything together:

\[
I = \int_{0}^{2} x^{-1/2}(2-x)^{-1/2} \cos( \sqrt{x(2-x)} ) dx
\]
\[
= \int_{0}^{\pi/2} \left[ \frac{1}{2 \sin\theta \cos\theta} \right] \cos(2 \sin\theta \cos\theta) \cdot 4\sin\theta \cos\theta d\theta
\]
\[
= 2 \int_0^{\pi/2} \cos( \sin 2\theta ) d\theta
\]
Because 

- \( \sin 2\theta = 2\sin\theta \cos\theta \)
- The denominator cancels two of the numerator

But the argument in the cosine is \( \sin 2\theta \), not \( 2\sin\theta \cos\theta \). But \( 2\sin\theta\cos\theta = \sin 2\theta \).

So the integral simplifies to:

\[
I = 2 \int_0^{\pi/2} \cos(\sin 2\theta) d\theta
\]

---

### Step 2: Analytical Evaluation

Let’s use the substitution \( \phi = 2\theta \). Then

- \( \theta = \phi/2 \)
- \( d\theta = d\phi/2 \)
- When \( \theta = 0 \), \( \phi = 0 \)
- When \( \theta = \pi/2 \), \( \phi = \pi \)

So,

\[
I = 2 \int_0^{\pi/2} \cos(\sin 2\theta) d\theta
= 2 \int_{0}^{\pi} \cos(\sin \phi) \cdot \frac{1}{2} d\phi
= \int_0^{\pi} \cos(\sin \phi) d\phi
\]

Thus,

\[
I = \int_0^{\pi} \cos(\sin \phi) d\phi
\]

---

### Step 3: Expressing in terms of Bessel functions

Recall the integral representation:

\[
\int_{0}^{\pi} \cos(a \sin x) dx = \pi J_0(a)
\]

where \( J_0 \) is the Bessel function of the first kind.

In our case, \( a = 1 \):

\[
I = \pi J_0(1)
\]

---

### Step 4: Numerical approximation

The value of \( J_0(1) \):

\[
J_0(1) \approx 0.7651976866
\]
So,
\[
I \approx \pi \times 0.7651976866 \approx 2.4048255577
\]
So, to 10 decimal places:

\[
I \approx 2.4048255577
\]

---

### Step 5: JSON Output

```json
{"answer": "\\pi J_0(1)", "numerical_answer": "2.4048255577"}
```