To compute the definite integral \(\int_0^{\frac{\pi}{2}} x \ln(\sin x) \, dx\), we will follow these steps:

### Step 1: Use a known result and symmetry
The integral \(\int_0^{\frac{\pi}{2}} \ln(\sin x) \, dx\) is a well-known result:
\[
\int_0^{\frac{\pi}{2}} \ln(\sin x) \, dx = -\frac{\pi}{2} \ln 2.
\]
However, our integral includes an additional factor of \(x\). To handle this, we can use integration by parts or exploit symmetry and known series expansions.

### Step 2: Express \(\ln(\sin x)\) as a series
We can express \(\ln(\sin x)\) using its Fourier series expansion:
\[
\ln(\sin x) = -\ln 2 - \sum_{k=1}^\infty \frac{\cos(2kx)}{k}, \quad 0 < x < \pi.
\]
Thus, the integral becomes:
\[
\int_0^{\frac{\pi}{2}} x \ln(\sin x) \, dx = -\ln 2 \int_0^{\frac{\pi}{2}} x \, dx - \sum_{k=1}^\infty \frac{1}{k} \int_0^{\frac{\pi}{2}} x \cos(2kx) \, dx.
\]

### Step 3: Compute the integrals
First, compute the simple integral:
\[
\int_0^{\frac{\pi}{2}} x \, dx = \frac{\pi^2}{8}.
\]
Next, compute the integral involving \(\cos(2kx)\) using integration by parts:
\[
\int x \cos(2kx) \, dx = \frac{x \sin(2kx)}{2k} + \frac{\cos(2kx)}{4k^2} + C.
\]
Evaluating from \(0\) to \(\frac{\pi}{2}\):
\[
\int_0^{\frac{\pi}{2}} x \cos(2kx) \, dx = \left. \frac{x \sin(2kx)}{2k} \right|_0^{\frac{\pi}{2}} + \left. \frac{\cos(2kx)}{4k^2} \right|_0^{\frac{\pi}{2}} = \frac{\pi \sin(k\pi)}{4k} + \frac{\cos(k\pi) - 1}{4k^2}.
\]
Since \(\sin(k\pi) = 0\) for integer \(k\), and \(\cos(k\pi) = (-1)^k\), this simplifies to:
\[
\int_0^{\frac{\pi}{2}} x \cos(2kx) \, dx = \frac{(-1)^k - 1}{4k^2}.
\]

### Step 4: Sum the series
Now, the integral becomes:
\[
\int_0^{\frac{\pi}{2}} x \ln(\sin x) \, dx = -\frac{\pi^2}{8} \ln 2 - \sum_{k=1}^\infty \frac{(-1)^k - 1}{4k^3}.
\]
Notice that \((-1)^k - 1\) is \(-2\) for odd \(k\) and \(0\) for even \(k\). Thus, the sum simplifies to:
\[
\sum_{k=1}^\infty \frac{(-1)^k - 1}{4k^3} = -\frac{1}{2} \sum_{m=1}^\infty \frac{1}{(2m-1)^3}.
\]
The sum of the reciprocals of the odd cubes is related to the Riemann zeta function and Catalan's constant, but it can be expressed as:
\[
\sum_{m=1}^\infty \frac{1}{(2m-1)^3} = \frac{7}{8} \zeta(3).
\]
Thus:
\[
\int_0^{\frac{\pi}{2}} x \ln(\sin x) \, dx = -\frac{\pi^2}{8} \ln 2 + \frac{7}{16} \zeta(3).
\]

### Step 5: Numerical approximation
The exact answer is:
\[
-\frac{\pi^2}{8} \ln 2 + \frac{7}{16} \zeta(3).
\]
Numerically:
\[
-\frac{\pi^2}{8} \ln 2 \approx -0.5993118626,
\]
\[
\frac{7}{16} \zeta(3) \approx 0.5258998951,
\]
\[
\text{Total} \approx -0.5993118626 + 0.5258998951 = -0.0734119675.
\]

### Final Answer
```json
{"answer": "-\\frac{\\pi^2}{8} \\ln 2 + \\frac{7}{16} \\zeta(3)", "numerical_answer": "-0.0734119675"}
```