<think>
Okay, let's tackle this integral step by step. The integral given is ∫₀² x^(1/2) (2 - x)^(-1/2) cos(1.0√(x(2 - x))) dx. Hmm, that looks a bit complicated, but maybe a substitution can simplify it.

First, I notice that the integrand has x and (2 - x) terms, which makes me think of a substitution that can symmetrize the expression. Let me try substituting t = x - 1. That way, the limits when x=0 would be t=-1, and x=2 would be t=1. But I'm not sure if that helps directly. Alternatively, maybe a trigonometric substitution? Since there's a square root of x(2 - x), which resembles the form of sin²θ or something similar.

Wait, x(2 - x) can be rewritten as 2x - x² = -(x² - 2x) = -(x² - 2x +1 -1) = -(x -1)^2 +1. So, that's 1 - (x -1)^2. That looks like the identity 1 - sin²θ = cos²θ. So maybe substituting x -1 = sinθ? Let's try that.

Let’s set x = 1 + sinθ. Then, dx = cosθ dθ. When x=0, sinθ = -1, so θ = -π/2. When x=2, sinθ = 1, so θ = π/2. Let's substitute into the integral.

First, compute x^(1/2): (1 + sinθ)^(1/2). Then (2 - x)^(-1/2) is (2 - (1 + sinθ))^(-1/2) = (1 - sinθ)^(-1/2). The argument of the cosine is 1.0√(x(2 - x)) = √[(1 + sinθ)(1 - sinθ)] = √(1 - sin²θ) = cosθ. So the cosine term becomes cos(1.0 * cosθ) = cos(cosθ).

Putting it all together, the integral becomes:

∫ from θ=-π/2 to θ=π/2 of [ (1 + sinθ)^(1/2) * (1 - sinθ)^(-1/2) * cosθ ] * cos(cosθ) dθ.

Simplify the terms inside the integrand:

(1 + sinθ)^(1/2) / (1 - sinθ)^(1/2) = sqrt( (1 + sinθ)/(1 - sinθ) )

Multiply numerator and denominator by (1 + sinθ)^(1/2):

sqrt( (1 + sinθ)^2 / (1 - sin²θ) ) = sqrt( (1 + sinθ)^2 / cos²θ ) = (1 + sinθ)/cosθ.

So the integrand simplifies to:

(1 + sinθ)/cosθ * cosθ * cos(cosθ) dθ = (1 + sinθ) cos(cosθ) dθ.

Therefore, the integral becomes ∫ from -π/2 to π/2 (1 + sinθ) cos(cosθ) dθ.

Hmm, that's simpler. Let's split the integral into two parts:

∫ (1 + sinθ) cos(cosθ) dθ = ∫ cos(cosθ) dθ + ∫ sinθ cos(cosθ) dθ.

Let's consider the first integral, ∫ cos(cosθ) dθ from -π/2 to π/2. The integrand is an even function because cos(cos(-θ)) = cos(cosθ), and the limits are symmetric. So this becomes 2 ∫₀^{π/2} cos(cosθ) dθ.

The second integral is ∫ sinθ cos(cosθ) dθ from -π/2 to π/2. Here, sinθ is an odd function, and cos(cosθ) is even. The product is odd, so the integral over symmetric limits is zero. Therefore, the second integral cancels out.

So the entire integral reduces to 2 ∫₀^{π/2} cos(cosθ) dθ.

Wait, but that seems familiar. The integral of cos(cosθ) from 0 to π/2 is a known form related to Bessel functions. Specifically, the integral representation of the Bessel function J₀(1) is (1/π) ∫₀^π cos(cosθ) dθ. But our integral is from 0 to π/2. Let me check.

The standard integral is J₀(x) = (1/π) ∫₀^π cos(x cosθ) dθ. For x=1, J₀(1) = (1/π) ∫₀^π cos(cosθ) dθ. Therefore, ∫₀^π cos(cosθ) dθ = π J₀(1). But our integral is from 0 to π/2. However, since cos(cosθ) is symmetric around θ=π/2 in the interval [0, π], maybe ∫₀^{π/2} cos(cosθ) dθ = (1/2) ∫₀^π} cos(cosθ) dθ = (π/2) J₀(1). Wait, but is that true?

Wait, no. The integral from 0 to π/2 is not exactly half of the integral from 0 to π. Let me compute ∫₀^{π} cos(cosθ) dθ = 2 ∫₀^{π/2} cos(cosθ) dθ. Because cos(cosθ) is symmetric around θ=π/2. Wait, cos(cosθ) from θ=0 to π. Let’s substitute φ = π - θ in the integral from π/2 to π. Then, cos(cos(π - φ)) = cos(-cosφ) = cos(cosφ). So the integral from π/2 to π is the same as from 0 to π/2. Therefore, ∫₀^π cos(cosθ) dθ = 2 ∫₀^{π/2} cos(cosθ) dθ. Therefore, ∫₀^{π/2} cos(cosθ) dθ = (1/2) ∫₀^π cos(cosθ) dθ = (π/2) J₀(1).

Therefore, our original integral is 2 * (π/2) J₀(1) = π J₀(1).

So the exact value of the integral is π J₀(1), where J₀ is the Bessel function of the first kind of order 0.

Therefore, the exact answer is π J₀(1). Now, we need to compute the numerical approximation. The Bessel function J₀(1) has a known value. Let me recall that J₀(1) ≈ 0.7651976866. Therefore, multiplying by π gives approximately 0.7651976866 * 3.1415926536 ≈ 2.403787642.

Wait, let me check that. Let me compute J₀(1) more accurately. Using a calculator or table, J₀(1) is approximately 0.7651976865579666. So π times that is approximately 0.7651976865579666 * 3.141592653589793 ≈ 2.403787642293542.

Rounded to 10 decimal places, that's 2.4037876423.

Therefore, the exact answer is π J₀(1), and the numerical approximation is approximately 2.4037876423.

But let me verify the steps are correct. Let's recap:

Original integral: ∫₀² x^(1/2) (2 - x)^(-1/2) cos(√(x(2 - x))) dx.

Substitution x = 1 + sinθ, leading to the integral becoming 2 ∫₀^{π/2} cos(cosθ) dθ, which equals π J₀(1). That seems correct. The key step was recognizing the integral of cos(cosθ) over 0 to π/2 relates to the Bessel function. Since J₀(1) is (1/π) ∫₀^π cos(cosθ) dθ, then ∫₀^π cos(cosθ) dθ = π J₀(1), and ∫₀^{π/2} cos(cosθ) dθ = (π/2) J₀(1). Then multiplying by 2 gives π J₀(1). So the exact answer is π J₀(1).

Therefore, the exact answer in LaTeX is \pi J_0(1), but since Bessel functions are standard, we can write it as \pi J_0(1). However, sometimes people prefer to write it using the Bessel function notation. Alternatively, if there's a more elementary form, but I don't think so. The integral doesn't seem to simplify further in terms of elementary functions. So the exact answer is π times the Bessel function of the first kind of order 0 evaluated at 1.

Therefore, the numerical value is approximately 2.4037876423 when rounded to 10 decimal places.
</think>

{"answer": "\\pi J_0(1)", "numerical_answer": "2.4037876423"}