
To solve the definite integral \(\int_0^1 \left( e^{e^x} - e^{e^x - x} \right) dx\), we proceed as follows:

### Step 1: Identify the Antiderivative
We need to find a function \(F(x)\) whose derivative is the integrand \(e^{e^x} - e^{e^x - x}\). Consider the function \(F(x) = e^{e^x - x}\). Let's compute its derivative:
\[
F'(x) = \frac{d}{dx} \left( e^{e^x - x} \right) = e^{e^x - x} \cdot \frac{d}{dx} \left( e^x - x \right) = e^{e^x - x} \cdot (e^x - 1)
\]
Expanding this, we get:
\[
F'(x) = e^{e^x - x} \cdot e^x - e^{e^x - x} = e^{e^x} - e^{e^x - x}
\]
This matches the integrand exactly. Thus, \(F(x) = e^{e^x - x}\) is the antiderivative.

### Step 2: Evaluate the Definite Integral
Using the Fundamental Theorem of Calculus, the definite integral from \(0\) to \(1\) is:
\[
\int_0^1 \left( e^{e^x} - e^{e^x - x} \right) dx = F(1) - F(0)
\]
Substituting the bounds:
\[
F(1) = e^{e^1 - 1} = e^{e - 1}, \quad F(0) = e^{e^0 - 0} = e^{1 - 0} = e
\]
Thus, the integral simplifies to:
\[
e^{e - 1} - e
\]

### Step 3: Numerical Approximation
To approximate \(e^{e - 1} - e\) numerically:
- \(e \approx 2.718281828459045\)
- \(e - 1 \approx 1.718281828459045\)
- \(e^{e - 1} \approx e^{1.718281828459045} \approx 5.574941541322659\)
- Subtracting \(e\) gives \(5.574941541322659 - 2.718281828459045 \approx 2.856659712863614\)

Rounded to 10 decimal places, the numerical approximation is \(2.8566597129\).

{"answer": "e^{e - 1} - e", "numerical_answer": "2.8566597129"}