Let's break down and solve the integral:
\[
I = \int_{\frac{1}{8}}^{\frac{1}{4}} \frac{\ln(2x)\ln(4x)\ln(8x)}{x} \,dx
\]

### Step 1: Expand each logarithm

- \(\ln(2x) = \ln 2 + \ln x\)
- \(\ln(4x) = \ln 4 + \ln x = 2\ln 2 + \ln x\)
- \(\ln(8x) = \ln 8 + \ln x = 3\ln 2 + \ln x\)

So,
\[
I = \int_{\frac{1}{8}}^{\frac{1}{4}} \frac{(\ln 2 + \ln x)(2\ln 2 + \ln x)(3\ln 2 + \ln x)}{x} \,dx
\]

### Step 2: Expand out the product

Let \(A = \ln 2\), then the integrand becomes:
\[
(\ln 2 + \ln x)(2\ln 2 + \ln x)(3\ln 2 + \ln x)
\]

Use the multinomial expansion:

\[
(a+b)(c+b)(d+b) = (a)(c)(d) + (a)(c)b + (a)b(d) + (a)b(b) + b(c)(d) + b(c)b + b(b)(d) + b^3
\]
but here, with repeated b's, but easier to expand systematically.

Let's expand step by step:

First, expand \((A + \ln x)(2A + \ln x)\):
\[
= (A)(2A) + (A)(\ln x) + (\ln x)(2A) + (\ln x)(\ln x) \\
= 2A^2 + A\ln x + 2A\ln x + (\ln x)^2 \\
= 2A^2 + 3A\ln x + (\ln x)^2
\]

Now, multiply this with \((3A + \ln x)\):

\[
\Big[2A^2 + 3A\ln x + (\ln x)^2\Big](3A + \ln x) \\
= 2A^2(3A + \ln x) + 3A\ln x(3A + \ln x) + (\ln x)^2(3A + \ln x) \\
= 2A^2\cdot3A + 2A^2\ln x + 3A\ln x\cdot 3A + 3A\ln x\cdot \ln x \\
\qquad + (\ln x)^2\cdot 3A + (\ln x)^3 \\
= 6A^3 + 2A^2\ln x + 9A^2\ln x + 3A(\ln x)^2 + 3A(\ln x)^2 + (\ln x)^3 \\
\]

But let's check: \(2A^2 \cdot \ln x = 2A^2\ln x\), and \(3A \ln x \cdot 3A = 9A^2\ln x\).

But actually, more carefully:

- \(2A^2(3A) = 6A^3\)
- \(2A^2(\ln x) = 2A^2\ln x\)
- \(3A\ln x(3A) = 9A^2\ln x\)
- \(3A\ln x(\ln x) = 3A\ln x\cdot\ln x = 3A(\ln x)^2\)
- \((\ln x)^2(3A) = 3A(\ln x)^2\)
- \((\ln x)^2(\ln x) = (\ln x)^3\)

So sum these up:

- Constant: \(6A^3\)
- \(\ln x\) terms: \(2A^2\ln x + 9A^2\ln x = 11A^2\ln x\)
- \((\ln x)^2\) terms: \(3A(\ln x)^2 + 3A(\ln x)^2 = 6A(\ln x)^2\)
- \((\ln x)^3\) term: \((\ln x)^3\)

So

\[
I = \int_{\frac{1}{8}}^{\frac{1}{4}} \frac{6A^3 + 11A^2 \ln x + 6A(\ln x)^2 + (\ln x)^3}{x} \, dx
\]

Recall \(A = \ln 2\):

### Step 3: Integrate each term

Recall:
\[
\int \frac{(\ln x)^n}{x} dx = \frac{(\ln x)^{n+1}}{n+1} + C
\]

So:

- \(\int \frac{1}{x} dx = \ln x\)
- \(\int \frac{\ln x}{x} dx = \frac{1}{2}(\ln x)^2\)
- \(\int \frac{(\ln x)^2}{x} dx = \frac{1}{3}(\ln x)^3\)
- \(\int \frac{(\ln x)^3}{x} dx = \frac{1}{4}(\ln x)^4\)

So integrating term by term:

\[
\int \frac{6A^3}{x} dx = 6A^3 \ln x
\]
\[
\int \frac{11A^2 \ln x}{x} dx = 11A^2 \cdot \frac{1}{2} (\ln x)^2 = \frac{11}{2}A^2 (\ln x)^2
\]
\[
\int \frac{6A (\ln x)^2}{x} dx = 6A \cdot \frac{1}{3} (\ln x)^3 = 2A (\ln x)^3
\]
\[
\int \frac{(\ln x)^3}{x} dx = \frac{1}{4} (\ln x)^4
\]

So the indefinite integral is:

\[
F(x) = 6A^3 \ln x + \frac{11}{2}A^2 (\ln x)^2 + 2A (\ln x)^3 + \frac{1}{4}(\ln x)^4
\]

### Step 4: Evaluate at limits

So,
\[
I = F\left(\frac{1}{4}\right) - F\left(\frac{1}{8}\right)
\]

Now, compute \(\ln \frac{1}{4} = -\ln 4 = -2\ln 2 = -2A\)

and \(\ln \frac{1}{8} = -\ln 8 = -3\ln 2 = -3A\)

Now, substitute into the expression:

Let's compute \(F\left(\frac{1}{4}\right)\):

- \(\ln x = -2A\)
- \((\ln x)^2 = 4A^2\)
- \((\ln x)^3 = -8A^3\)
- \((\ln x)^4 = 16A^4\)

So,
\[
F\left(\frac{1}{4}\right) = 6A^3(-2A) + \frac{11}{2}A^2 (4A^2) + 2A(-8A^3) + \frac{1}{4} \cdot 16A^4
\]

Calculate each term:
- \(6A^3(-2A) = -12A^4\)
- \(\frac{11}{2}A^2 \cdot 4A^2 = 22A^4\)
- \(2A \cdot (-8A^3) = -16A^4\)
- \(\frac{1}{4} \cdot 16A^4 = 4A^4\)

So sum:

\[
F\left(\frac{1}{4}\right) = -12A^4 + 22A^4 - 16A^4 + 4A^4 = (-12 + 22 - 16 + 4)A^4 = (-2)A^4
\]

Now, for \(x = \frac{1}{8}\):

- \(\ln x = -3A\)
- \((\ln x)^2 = 9A^2\)
- \((\ln x)^3 = -27A^3\)
- \((\ln x)^4 = 81A^4\)

So,

\[
F\left(\frac{1}{8}\right) = 6A^3(-3A) + \frac{11}{2}A^2(9A^2) + 2A(-27A^3) + \frac{1}{4}(81A^4)
\]

Each term:

- \(6A^3 \cdot -3A = -18A^4\)
- \(\frac{11}{2}A^2 \cdot 9A^2 = \frac{99}{2}A^4\)
- \(2A \cdot -27A^3 = -54A^4\)
- \(\frac{1}{4} \cdot 81A^4 = 20.25A^4\)

Now sum:

- \(-18A^4 + \frac{99}{2}A^4 - 54A^4 + 20.25A^4\)
- \(\frac{99}{2} = 49.5\)
- So
  \[
  -18 + 49.5 - 54 + 20.25 = (49.5 + 20.25) - (18 + 54) = 69.75 - 72 = -2.25
  \]
So,

\[
F\left(\frac{1}{8}\right) = -2.25A^4
\]

Therefore,

\[
I = F\left(\frac{1}{4}\right) - F\left(\frac{1}{8}\right)
= (-2A^4) - (-2.25A^4) = (0.25)A^4 = \frac{1}{4} (\ln 2)^4
\]

### Step 5: Compute numerical value

- \(\ln 2 \approx 0.6931471805599453\)
- So, \((\ln 2)^4 \approx (0.6931471805599453)^4 \approx 0.2310490601866484\)
- Then, dividing by 4: \(0.2310490601866484 / 4 = 0.0577622650466621\)

Rounded to 10 decimal places: **0.0577622650**

### Final Answer (JSON):

```json
{"answer": "\\frac{1}{4} (\\ln 2)^4", "numerical_answer": "0.0577622650"}
```