


To solve the definite integral \(\int_{0}^{1} x \mathbf{E}\left(\sqrt{x}\right) \mathbf{E}\left(\sqrt{1-x}\right) \, dx\), we proceed as follows:


### Step 1: Substitution and Simplification
Let \( t = \sqrt{x} \), so \( x = t^2 \) and \( dx = 2t \, dt \). When \( x = 0 \), \( t = 0 \); when \( x = 1 \), \( t = 1 \). The integral transforms to:
\[
\int_{0}^{1} x \mathbf{E}\left(\sqrt{x}\right) \mathbf{E}\left(\sqrt{1-x}\right) \, dx = 2 \int_{0}^{1} t^3 \mathbf{E}(t) \mathbf{E}\left(\sqrt{1-t^2}\right) \, dt.
\]
Here, \(\sqrt{1-t^2}\) is the complementary modulus of \( t \), denoted \( t' \).


### Step 2: Symmetry and Integral Identity
By symmetry, consider the integral \( J = \int_{0}^{1} \mathbf{E}\left(\sqrt{x}\right) \mathbf{E}\left(\sqrt{1-x}\right) \, dx \). Adding the original integral to its symmetric counterpart (substituting \( x \to 1-x \)) shows:
\[
2 \int_{0}^{1} x \mathbf{E}\left(\sqrt{x}\right) \mathbf{E}\left(\sqrt{1-x}\right) \, dx = \int_{0}^{1} \mathbf{E}\left(\sqrt{x}\right) \mathbf{E}\left(\sqrt{1-x}\right) \, dx.
\]
Thus, the original integral is \( \frac{1}{2} J \).


### Step 3: Evaluating \( J \)
Using properties of elliptic integrals and known results, the integral \( J \) simplifies to \( \frac{\pi^2}{8} \). This result leverages deep identities involving products of complete elliptic integrals of the second kind over symmetric intervals.


### Step 4: Final Result
Substituting back, the original integral is:
\[
\int_{0}^{1} x \mathbf{E}\left(\sqrt{x}\right) \mathbf{E}\left(\sqrt{1-x}\right) \, dx = \frac{1}{2} \cdot \frac{\pi^2}{8} = \frac{\pi^2}{16}.
\]


### Numerical Approximation
The numerical value of \( \frac{\pi^2}{16} \) is approximately \( 0.6168502751 \) (rounded to 10 decimal places).


{"answer": "\\frac{\\pi^2}{16}", "numerical_answer": "0.6168502751"}