Let's proceed step by step:

**Step 1: Understanding \( H_3 \left( \sqrt{x(2-x)} \right) \)**
The physicist's Hermite polynomial of degree 3 is:
\[
H_3(y) = 8y^3 - 12y
\]

Thus,
\[
H_3(\sqrt{x(2-x)}) = 8(\sqrt{x(2-x)})^3 - 12\sqrt{x(2-x)} = 8(x(2-x))^{3/2} -12(x(2-x))^{1/2}
\]

**Step 2: Write the integral explicitly**
\[
I = \int_0^2 x H_3\left(\sqrt{x(2-x)}\right) dx = \int_0^2 x \left[8(x(2-x))^{3/2} - 12(x(2-x))^{1/2} \right] dx
\]
\[
= 8 \int_0^2 x (x(2-x))^{3/2} dx - 12 \int_0^2 x (x(2-x))^{1/2} dx
\]

Let’s call
\[
I_1 = \int_0^2 x (x(2-x))^{3/2} dx
\]
\[
I_2 = \int_0^2 x (x(2-x))^{1/2} dx
\]

So,
\[
I = 8I_1 - 12I_2
\]

---

**Step 3: Compute the sub-integrals**

### **Evaluate \( I_1 = \int_0^2 x (x(2-x))^{3/2} dx \)**
Let’s first expand \( (x(2-x))^{3/2} \):

Let’s use substitution:
Let \( x = 2 \sin^2 \theta \). When \( x = 0, \theta = 0 \). When \( x = 2, \sin^2 \theta = 1 \rightarrow \theta = \frac{\pi}{2} \).

Compute \( x(2-x) = 2\sin^2 \theta (2-2\sin^2 \theta) = 4\sin^2 \theta \cos^2 \theta = 4\sin^2 \theta \cos^2 \theta \).

Thus,
\(
(x(2-x))^{3/2} = (4 \sin^2 \theta \cos^2 \theta)^{3/2}
= 8 \sin^3 \theta \cos^3 \theta
\)

Also,
\(
x = 2 \sin^2 \theta
\)
and
\(
dx = 4 \sin \theta \cos \theta d\theta
= 2 \sin 2\theta d\theta
\)

So,
\[
I_1 = \int_{x=0}^{x=2} x (x(2-x))^{3/2} dx
= \int_{\theta=0}^{\theta=\frac{\pi}{2}} [2 \sin^2\theta][8 \sin^3\theta \cos^3 \theta] \cdot [4 \sin\theta \cos\theta] d\theta
\]

Multiply all together:
\[
2 \cdot 8 \cdot 4 = 64
\]
Powers:
\[
\sin^2\theta \times \sin^3\theta \times \sin\theta = \sin^6\theta
\]
\[
\cos^3\theta \times \cos\theta = \cos^4\theta
\]

So,
\[
I_1 = 64 \int_0^{\pi/2} \sin^6 \theta \cos^4 \theta d\theta
\]

### **Evaluate \( I_2 = \int_0^2 x (x(2-x))^{1/2} dx \)**
Similarly, \( (x(2-x))^{1/2} = 2 \sin \theta \cos \theta \)
So,
\[
I_2 = \int_{\theta=0}^{\theta=\frac{\pi}{2}} [2 \sin^2\theta][2 \sin\theta \cos\theta][4\sin\theta\cos\theta] d\theta
\]
\( 2 \times 2 \times 4 = 16 \)

Sines: \( \sin^2\theta \times \sin\theta \times \sin\theta = \sin^4\theta \)
Cosines: \( \cos\theta \times \cos\theta = \cos^2\theta \)

So,
\[
I_2 = 16 \int_0^{\pi/2} \sin^4\theta \cos^2\theta d\theta
\]

---

**Step 4: Plug \( I_1 \) and \( I_2 \) back**
\[
I = 8I_1 - 12I_2 = 8 \times 64 \int_0^{\pi/2} \sin^6\theta \cos^4\theta d\theta -12 \times 16 \int_0^{\pi/2} \sin^4\theta \cos^2\theta d\theta
\]
\[
I = 512 \int_0^{\pi/2} \sin^6\theta \cos^4\theta d\theta - 192 \int_0^{\pi/2} \sin^4\theta \cos^2\theta d\theta
\]

---

**Step 5: Express as Beta (or Gamma) functions**

Recall:
\[
\int_0^{\pi/2} \sin^p \theta \cos^q \theta d\theta = \frac{1}{2} \mathrm{B}\left(\frac{p+1}{2}, \frac{q+1}{2}\right) = \frac{\Gamma\left(\frac{p+1}{2}\right) \Gamma\left(\frac{q+1}{2}\right)}{2 \Gamma\left(\frac{p+q}{2}+1\right)}
\]

So,

- For \( \int_0^{\pi/2} \sin^6 \theta \cos^4 \theta d\theta \):
  - \( p = 6, q = 4 \)
  - \(
    \int = \frac{1}{2} \mathrm{B}\left(\frac{7}{2}, \frac{5}{2}\right)
    \)

- For \( \int_0^{\pi/2} \sin^4 \theta \cos^2 \theta d\theta \):
  - \( p = 4, q = 2 \)
  - \(
    \int = \frac{1}{2} \mathrm{B}\left(\frac{5}{2}, \frac{3}{2}\right)
    \)

So,

\[
I = 512 \cdot \frac{1}{2} \mathrm{B}\left(\frac{7}{2}, \frac{5}{2}\right) - 192 \cdot \frac{1}{2} \mathrm{B}\left(\frac{5}{2}, \frac{3}{2}\right)
\]
\[
= 256\, \mathrm{B}\left(\frac{7}{2}, \frac{5}{2}\right) - 96\, \mathrm{B}\left(\frac{5}{2}, \frac{3}{2}\right)
\]

Recall:
\[
\mathrm{B}(a, b) = \frac{\Gamma(a) \Gamma(b)}{\Gamma(a+b)}
\]

**Gamma function values:**
- \( \Gamma(\frac{3}{2}) = \frac{1}{2}\sqrt{\pi} \)
- \( \Gamma(\frac{5}{2}) = \frac{3}{4}\sqrt{\pi} \)
- \( \Gamma(\frac{7}{2}) = \frac{15}{8}\sqrt{\pi} \)
- \( \Gamma(\frac{9}{2}) = \frac{105}{16}\sqrt{\pi} \)

Let’s check for \( \Gamma(n+1/2) = (n-\frac{1}{2}) \cdots \frac{1}{2} \Gamma(\frac{1}{2}) \) and \( \Gamma(\frac{1}{2}) = \sqrt{\pi} \)

Let’s evaluate:
\[
\mathrm{B}\left(\frac{7}{2}, \frac{5}{2}\right) = \frac{\Gamma(\frac{7}{2})\Gamma(\frac{5}{2})}{\Gamma(7)}
\]
- \( \Gamma(7) = 6! = 720 \)
- \( \Gamma(\frac{7}{2}) = \frac{5}{2} \cdot \frac{3}{2} \cdot \frac{1}{2} \cdot \Gamma(\frac{1}{2}) = \frac{15}{8} \sqrt{\pi} \)
- \( \Gamma(\frac{5}{2}) = \frac{3}{2} \cdot \frac{1}{2} \cdot \Gamma(\frac{1}{2}) = \frac{3}{4} \sqrt{\pi} \)

So,
\[
\mathrm{B}\left(\frac{7}{2}, \frac{5}{2}\right)
= \frac{\frac{15}{8} \sqrt{\pi} \cdot \frac{3}{4} \sqrt{\pi}}{720}
= \frac{45}{32} \pi \div 720 = \frac{45 \pi}{32 \cdot 720} = \frac{45 \pi}{23040} = \frac{3 \pi}{1536}
\]

For the other term:
\[
\mathrm{B}\left(\frac{5}{2}, \frac{3}{2}\right) = \frac{\Gamma(\frac{5}{2})\Gamma(\frac{3}{2})}{\Gamma(4)}
\]
- \( \Gamma(4) = 3! = 6 \)
- \( \Gamma(\frac{3}{2}) = \frac{1}{2} \sqrt{\pi} \)

So,
\[
\mathrm{B}\left(\frac{5}{2}, \frac{3}{2}\right)
= \frac{ \frac{3}{4} \sqrt{\pi} \cdot \frac{1}{2} \sqrt{\pi} }{6 }
= \frac{3}{4} \cdot \frac{1}{2} = \frac{3}{8}
\]
So numerator: \( \frac{3}{8} \pi \), denominator: \( 6 \)
Total: \( \frac{3 \pi}{48} = \frac{\pi}{16} \)

**So the entire integral is:**
\[
I = 256 \cdot \frac{3\pi}{1536} - 96 \cdot \frac{\pi}{16}
\]
\[
256 \cdot \frac{3\pi}{1536} = \frac{768\pi}{1536} = \frac{\pi}{2}
\]
\[
96 \cdot \frac{\pi}{16} = 6\pi
\]

So,
\[
I = \frac{\pi}{2} - 6\pi = -\frac{11\pi}{2}
\]

---

**Step 6: Numerical value**

\[
-\frac{11\pi}{2} \approx -17.2787595947
\]
(using \(\pi \approx 3.1415926536\))

---

**Step 7: JSON Output**

```json
{"answer": "-\\frac{11\\pi}{2}", "numerical_answer": "-17.2787595947"}
```