We first need to locate where the expression inside the absolute value, 1 + 2 sin x, changes its sign. Set

  1 + 2 sin x = 0  ⟹  sin x = -1/2.

Within [0, 2π] sin x = -1/2 at x = 7π/6 and x = 11π/6.

Thus, the integral

  I = ∫₀^(2π)|1 + 2 sin x| dx

can be split as

  I = ∫₀^(7π/6)(1 + 2 sin x) dx + ∫_(7π/6)^(11π/6) –(1 + 2 sin x) dx + ∫_(11π/6)^(2π)(1 + 2 sin x) dx.

The antiderivative of 1 + 2 sin x is

  ∫(1 + 2 sin x)dx = x – 2 cos x.

Now, we calculate each piece:

1. For I₁ = ∫₀^(7π/6)(1 + 2 sin x)dx:
  I₁ = [x – 2 cos x]₀^(7π/6)
   = (7π/6 – 2 cos(7π/6)) – (0 – 2 cos 0)
   = 7π/6 – 2(–√3/2) + 2(1)
   = 7π/6 + √3 + 2.

2. For I₂ = ∫_(7π/6)^(11π/6) –(1 + 2 sin x)dx:
  I₂ = –[x – 2 cos x]_(7π/6)^(11π/6)
   = –[(11π/6 – 2 cos(11π/6)) – (7π/6 – 2 cos(7π/6))]
   = –[(11π/6 – 2(√3/2)) – (7π/6 – 2(–√3/2))]
   = –[(11π/6 – √3) – (7π/6 + √3)]
   = –[(4π/6 – 2√3)]
   = –(2π/3 – 2√3)
   = –2π/3 + 2√3.

3. For I₃ = ∫_(11π/6)^(2π)(1 + 2 sin x)dx:
  I₃ = [x – 2 cos x]_(11π/6)^(2π)
   = [2π – 2 cos 2π] – [11π/6 – 2 cos(11π/6)]
   = (2π – 2(1)) – [11π/6 – 2(√3/2)]
   = (2π – 2) – (11π/6 – √3)
   = 2π – 2 – 11π/6 + √3.
  Writing 2π as 12π/6 gives:
   = (12π/6 – 11π/6) – 2 + √3
   = π/6 – 2 + √3.

Now, adding I₁, I₂, and I₃ we obtain:
  I = (7π/6 + √3 + 2) + (–2π/3 + 2√3) + (π/6 – 2 + √3).

Combine the π-terms:
  (7π/6 – 2π/3 + π/6) = [7π/6 – 4π/6 + π/6] = 4π/6 = 2π/3.

Combine the constant terms:
  2 – 2 = 0.

Combine the √3 terms:
  (√3 + 2√3 + √3) = 4√3.

Thus, the exact value is

  I = 2π/3 + 4√3.

A numerical approximation is computed as follows:
  2π/3 ≈ 2 × 3.141592653589793 / 3 ≈ 2.0943951023931953,
  4√3 ≈ 4 × 1.7320508075688772 ≈ 6.928203230275509,
  I ≈ 2.0943951023931953 + 6.928203230275509 ≈ 9.022598332668705.

Rounded to 10 decimal places, I ≈ 9.0225983327.

{"answer": "$\\frac{2\\pi}{3} + 4\\sqrt{3}$", "numerical_answer": "9.0225983327"}