To compute the definite integral \(\int_{0}^{1} \arcsin(x) \arccos(x) \, dx\), we can follow these steps:

### Step 1: Simplify the Integrand
First, observe that \(\arcsin(x) + \arccos(x) = \frac{\pi}{2}\) for all \(x \in [-1, 1]\). Therefore, we can express \(\arccos(x)\) as:
\[
\arccos(x) = \frac{\pi}{2} - \arcsin(x).
\]
Substituting this into the integrand:
\[
\arcsin(x) \arccos(x) = \arcsin(x) \left(\frac{\pi}{2} - \arcsin(x)\right) = \frac{\pi}{2} \arcsin(x) - \arcsin^2(x).
\]
Thus, the integral becomes:
\[
\int_{0}^{1} \arcsin(x) \arccos(x) \, dx = \frac{\pi}{2} \int_{0}^{1} \arcsin(x) \, dx - \int_{0}^{1} \arcsin^2(x) \, dx.
\]

### Step 2: Compute \(\int \arcsin(x) \, dx\)
Using integration by parts:
\[
\int \arcsin(x) \, dx = x \arcsin(x) - \int \frac{x}{\sqrt{1 - x^2}} \, dx.
\]
The second integral is straightforward:
\[
\int \frac{x}{\sqrt{1 - x^2}} \, dx = -\sqrt{1 - x^2} + C.
\]
Thus:
\[
\int \arcsin(x) \, dx = x \arcsin(x) + \sqrt{1 - x^2} + C.
\]
Evaluating from 0 to 1:
\[
\left. x \arcsin(x) + \sqrt{1 - x^2} \right|_{0}^{1} = \left(1 \cdot \frac{\pi}{2} + 0\right) - (0 + 1) = \frac{\pi}{2} - 1.
\]

### Step 3: Compute \(\int \arcsin^2(x) \, dx\)
Using integration by parts:
\[
\int \arcsin^2(x) \, dx = x \arcsin^2(x) - \int \frac{2x \arcsin(x)}{\sqrt{1 - x^2}} \, dx.
\]
For the second integral, let \(u = \arcsin(x)\), \(du = \frac{1}{\sqrt{1 - x^2}} dx\), and \(dv = \frac{2x}{\sqrt{1 - x^2}} dx\), \(v = -2\sqrt{1 - x^2}\):
\[
\int \frac{2x \arcsin(x)}{\sqrt{1 - x^2}} \, dx = -2\sqrt{1 - x^2} \arcsin(x) + 2 \int \sqrt{1 - x^2} \cdot \frac{1}{\sqrt{1 - x^2}} \, dx = -2\sqrt{1 - x^2} \arcsin(x) + 2x + C.
\]
Thus:
\[
\int \arcsin^2(x) \, dx = x \arcsin^2(x) + 2\sqrt{1 - x^2} \arcsin(x) - 2x + C.
\]
Evaluating from 0 to 1:
\[
\left. x \arcsin^2(x) + 2\sqrt{1 - x^2} \arcsin(x) - 2x \right|_{0}^{1} = \left(\frac{\pi^2}{4} + 0 - 2\right) - (0 + 0 - 0) = \frac{\pi^2}{4} - 2.
\]

### Step 4: Combine the Results
Substituting the results from Step 2 and Step 3 into the original expression:
\[
\int_{0}^{1} \arcsin(x) \arccos(x) \, dx = \frac{\pi}{2} \left(\frac{\pi}{2} - 1\right) - \left(\frac{\pi^2}{4} - 2\right) = \frac{\pi^2}{4} - \frac{\pi}{2} - \frac{\pi^2}{4} + 2 = 2 - \frac{\pi}{2}.
\]

### Numerical Approximation
The exact answer is \(2 - \frac{\pi}{2}\). Numerically:
\[
2 - \frac{\pi}{2} \approx 2 - 1.5707963268 = 0.4292036732.
\]

### Final Answer
```json
{"answer": "2 - \\frac{\\pi}{2}", "numerical_answer": "0.4292036732"}
```