We start with the integral

  I = ∫₀⁷ (∛(√(x²+1)+x) − ∛(√(x²+1)−x)) dx.

Step 1. Write the cube roots in a simpler form:
Let
  A = ∛(√(x²+1)+x)  and  B = ∛(√(x²+1)−x).
Then
  A³ = √(x²+1) + x  and  B³ = √(x²+1) − x.
Notice that
  A³ − B³ = 2x    and  A³ + B³ = 2√(x²+1).
Also, the product is
  A·B = ∛[(√(x²+1)+x)(√(x²+1)−x)] = ∛(x²+1 − x²) = ∛(1) = 1.

Step 2. Set u = A − B. Then by the cube formula,
  u³ = A³ - B³ - 3AB(A - B) = 2x - 3u,
so that
  u³ + 3u = 2x  ⟹  x = (u³ + 3u) / 2.

Differentiate with respect to u:
  dx/du = (3u² + 3) / 2 = (3/2)(u²+1)  ⟹  dx = (3/2)(u²+1) du.

Step 3. Change the limits:
• When x = 0, then
  A = ∛(√(0+1)+0) = 1  and  B = 1, so u = 1−1 = 0.
• When x = 7, u satisfies:
  2(7) = u³ + 3u  ⟹  u³ + 3u − 14 = 0.
Testing u = 2: 2³ + 3·2 − 14 = 8 + 6 − 14 = 0. Thus, u = 2.

Step 4. Express the integral in terms of u:
  I = ∫ (from x=0 to 7) u · dx = ∫ (from u=0 to 2) u · (3/2)(u²+1) du = (3/2) ∫₀² u(u²+1) du.
Expanding the integrand:
  u(u²+1) = u³ + u.
Thus,
  I = (3/2) ∫₀² (u + u³) du.

Step 5. Compute the antiderivative:
  ∫ (u + u³) du = (1/2)u² + (1/4)u⁴.
Evaluate from u=0 to u=2:
At u = 2, (1/2)(4) + (1/4)(16) = 2 + 4 = 6.
At u = 0, the value is 0.
Thus,
  I = (3/2) × 6 = 9.

Step 6. The exact answer is 9 and the numerical approximation is 9.0000000000.

{"answer": "$9$", "numerical_answer": "9.0000000000"}