Let's proceed step by step:

**Step 1: Rewrite the integral**

The integral is:
\[
I = \int_{0}^{2} x^{-1/2} (2-x)^{-1/2} \left[ 1 - 0.5x(2-x) \right] \, dx
\]

Let's expand inside the square brackets:
\[
1 - 0.5x(2-x) = 1 - 0.5(2x - x^2) = 1 - x + 0.5x^2
\]

So the integral becomes:
\[
I = \int_{0}^{2} x^{-1/2} (2-x)^{-1/2} (1 - x + 0.5x^2) \, dx
\]

This can be written as the sum of three integrals:
\[
I = \int_{0}^{2} x^{-1/2} (2-x)^{-1/2} \, dx
- \int_{0}^{2} x^{1/2} (2-x)^{-1/2} \, dx
+ 0.5 \int_{0}^{2} x^{3/2} (2-x)^{-1/2} \, dx
\]

Let's denote:
\[
I_1 = \int_{0}^{2} x^{-1/2} (2-x)^{-1/2} \, dx
\]
\[
I_2 = \int_{0}^{2} x^{1/2} (2-x)^{-1/2} \, dx
\]
\[
I_3 = \int_{0}^{2} x^{3/2} (2-x)^{-1/2} \, dx
\]

So:
\[
I = I_1 - I_2 + 0.5 I_3
\]

---

**Step 2: Express each integral in terms of Beta functions**

Recall:
\[
\int_0^a x^{p-1}(a-x)^{q-1} \, dx = a^{p+q-1} B(p,q) = a^{p+q-1} \frac{\Gamma(p)\Gamma(q)}{\Gamma(p+q)}
\]

So, for \( a = 2 \):

**For I₁:**
\[
I_1 = \int_{0}^{2} x^{-1/2}(2-x)^{-1/2}dx
\]
Here, \(p = \frac{1}{2}, q = \frac{1}{2}\), so \(p+q-1 = 0\):
\[
I_1 = 2^0 B\left(\frac12, \frac12\right) = B\left(\frac12, \frac12\right)
\]
But \(B\left(\frac12, \frac12\right) = \frac{\Gamma\left(\frac12\right)^2}{\Gamma(1)} = \frac{(\sqrt{\pi})^2}{1} = \pi\).
Thus,
\[
I_1 = \pi
\]

---

**For I₂:**

Let’s write:
\[
I_2 = \int_{0}^{2} x^{1/2} (2-x)^{-1/2} dx
\]
Here, \(p = \frac{3}{2}, q = \frac{1}{2}\), \(p+q-1 = 1\):
\[
I_2 = 2^1 B\left(\frac32, \frac12\right) = 2\cdot B\left(\frac32, \frac12\right)
\]

Calculate \(B\left(\frac32, \frac12\right)\):
\[
B\left(\frac32, \frac12\right) = \frac{\Gamma\left(\frac32\right)\Gamma\left(\frac12\right)}{\Gamma(2)}
\]
Recall:
\[
\Gamma\left(\frac12\right) = \sqrt{\pi}, \quad \Gamma(2) = 1!
\Gamma\left(\frac32\right) = \frac{1}{2}\Gamma\left(\frac12\right) = \frac{1}{2}\sqrt{\pi}
\]
So,
\[
B\left(\frac32, \frac12\right) = \frac{\frac12\sqrt{\pi} \cdot \sqrt{\pi}}{1} = \frac12\pi
\]
Thus,
\[
I_2 = 2 \cdot \frac12\pi = \pi
\]

---

**For I₃:**

\[
I_3 = \int_{0}^{2} x^{3/2} (2-x)^{-1/2} dx
\]
Here, \(p = \frac{5}{2}, q = \frac12\), so \(p+q-1 = 2\):
\[
I_3 = 2^2 B\left(\frac52, \frac12\right) = 4B\left(\frac52, \frac12\right)
\]

Calculate \(B\left(\frac52, \frac12\right)\):
\[
B\left(\frac52, \frac12\right) = \frac{\Gamma\left(\frac52\right)\Gamma\left(\frac12\right)}{\Gamma(3)}
\]
\[
\Gamma(3) = 2!
\]
To calculate \(\Gamma\left(\frac52\right)\):

\[
\Gamma\left(\frac52\right) = \left(\frac32\right)\Gamma\left(\frac32\right)
\]
But \(\Gamma\left(\frac32\right) = \frac12\sqrt{\pi}\), so:
\[
\Gamma\left(\frac52\right) = \frac32 \cdot \frac12\sqrt{\pi} = \frac34 \sqrt{\pi}
\]

Now,
\[
B\left(\frac52, \frac12\right) = \frac{\frac34\sqrt{\pi} \cdot \sqrt{\pi}}{2} = \frac{3}{4} \cdot \frac{\pi}{2} = \frac{3\pi}{8}
\]
Therefore,
\[
I_3 = 4 \cdot \frac{3\pi}{8} = \frac{3\pi}{2}
\]

---

**Step 3: Sum up**

Recall
\[
I = I_1 - I_2 + 0.5 I_3
\]
\[
I = \pi - \pi + 0.5 \cdot \frac{3\pi}{2}
\]
\[
I = 0 + \frac{3\pi}{4} = \frac{3\pi}{4}
\]

---

**Step 4: Numerical value**

\[
\frac{3\pi}{4} \approx \frac{3 \times 3.1415926536}{4} \approx \frac{9.4247779608}{4} \approx 2.3561944902
\]

---

**Step 5: Output in JSON**

```json
{"answer": "\\frac{3\\pi}{4}", "numerical_answer": "2.3561944902"}
```