Let's solve the definite integral:
\[
I = \int_0^2 x^{-1/2}(2-x)^{1/2}\left[1-\frac{1}{2}x(2-x)\right]^{1/2}dx
\]

**Step 1: Substitution**

Let \( x = 2\sin^2\theta \) with \( \theta \in [0, \frac{\pi}{2}] \).

Then,
\[
dx = 4\sin\theta\cos\theta\, d\theta = 2\sin 2\theta\, d\theta \\
x^{-1/2} = (2\sin^2\theta)^{-1/2} = \frac{1}{\sqrt{2}\sin\theta} \\
2-x = 2-2\sin^2\theta = 2\cos^2\theta \implies (2-x)^{1/2} = \sqrt{2} \cos\theta
\]

Now, compute the argument of the square root:
\[
1 - \frac{1}{2}x(2-x) = 1 - \frac{1}{2}(2\sin^2\theta)(2\cos^2\theta) \\
= 1 - 2\sin^2\theta\cos^2\theta = 1 - \frac{1}{2}\sin^2 2\theta
\]
So,
\[
\left[1 - \frac{1}{2}x(2-x)\right]^{1/2} = \left[1 - \frac{1}{2} \sin^2 2\theta \right]^{1/2}
\]

Now substitute everything:
\[
I = \int_{\theta=0}^{\pi/2}
\frac{1}{\sqrt{2}\sin\theta} \cdot \sqrt{2}\cos\theta \cdot \left[ 1 - \frac{1}{2} \sin^2 2\theta \right]^{1/2}
\cdot 2\sin 2\theta\, d\theta
\]
Simplifying:
\[
\frac{1}{\sqrt{2}\sin\theta} \cdot \sqrt{2}\cos\theta = \frac{\cos\theta}{\sin\theta}
\]
And \( \sin 2\theta = 2\sin\theta\cos\theta \) so
\[
2\sin 2\theta = 4\sin\theta\cos\theta
\]

So the integrand becomes:
\[
\frac{\cos\theta}{\sin\theta} \left[1 - \frac{1}{2} \sin^2 2\theta\right]^{1/2} \cdot 4\sin\theta\cos\theta 
= 4\cos^2\theta \left[1 - \frac{1}{2}\sin^2 2\theta\right]^{1/2}
\]

So,
\[
I = \int_0^{\pi/2} 4\cos^2\theta \left[1 - \frac{1}{2}\sin^2 2\theta\right]^{1/2} d\theta
\]

**Step 2: Use Substitution for the Square Root**

Let’s let \( \phi = 2\theta \), so when \( \theta = 0 \), \( \phi = 0 \) and when \( \theta = \frac{\pi}{2} \), \( \phi = \pi \).

\[
d\phi = 2 d\theta \implies d\theta = \frac{d\phi}{2}
\]
\[
\cos\theta = \sqrt{\frac{1+\cos 2\theta}{2}} = \sqrt{\frac{1+\cos\phi}{2}}
\implies \cos^2\theta = \frac{1+\cos\phi}{2}
\]

So,
\[
I = \int_0^{\pi/2} 4\cos^2\theta \left[1 - \frac{1}{2}\sin^2 2\theta\right]^{1/2} d\theta \\
= \int_0^{\pi/2} 4\cos^2\theta \left[1 - \frac{1}{2}\sin^2 (2\theta)\right]^{1/2} d\theta \\
= \int_{\phi=0}^{\pi} 4 \cdot \frac{1+\cos\phi}{2} \cdot \left[1 - \frac{1}{2}\sin^2\phi \right]^{1/2} \cdot \frac{d\phi}{2}
\]
\[
= \int_0^{\pi} (1+\cos\phi) \left(1 - \frac{1}{2}\sin^2\phi\right)^{1/2} d\phi
\]

**Step 3: Expand and Separate the Integral**

\[
I = \int_0^{\pi} (1+\cos\phi)\left(1-\frac{1}{2}\sin^2\phi\right)^{1/2} d\phi \\
= \int_0^{\pi} \left(1-\frac{1}{2}\sin^2\phi\right)^{1/2} d\phi  
+ \int_0^{\pi} \cos\phi \left(1-\frac{1}{2}\sin^2\phi\right)^{1/2} d\phi
\]

Let’s deal with each separately.

#### First term:
\[
I_1 = \int_0^{\pi} \left(1-\frac{1}{2}\sin^2\phi\right)^{1/2} d\phi
\]

Notice that \( \left(1-\frac{1}{2}\sin^2\phi\right)^{1/2} \) is the integrand of the complete elliptic integral of the second kind, \( E(k) \), with \( k^2 = \frac{1}{2} \).

From the definition:
\[
E(k) = \int_0^{\pi/2} \sqrt{1-k^2 \sin^2\phi}\, d\phi
\]
So over \( [0,\pi] \),
\[
\int_0^\pi \sqrt{1-k^2\sin^2\phi} d\phi = 2 E(k)
\]
So,
\[
I_1 = 2 E\left( \frac{1}{\sqrt{2}} \right )
\]

#### Second term:
\[
I_2 = \int_0^{\pi} \cos\phi \left(1-\frac{1}{2}\sin^2\phi\right)^{1/2} d\phi
\]

Let’s use substitution:
Let \( u = \sin\phi \implies du = \cos\phi d\phi \), when \( \phi=0 \to u=0 \), \( \phi=\pi \to u=0 \), so the boundaries are the same.
So,
\[
I_2 = \int_{u=0}^{u=0} \sqrt{1-\frac{1}{2}u^2}\, du = 0
\]
Because the endpoints are the same and the path is traversed forward and then backward, the integrand is single-valued, the integral is 0.

**Step 4: Combine the Results**

So,
\[
I = I_1 + I_2 = 2 E\left(\frac{1}{\sqrt{2}}\right)
\]

**Step 5: Numerical Approximation**

The value of \( E\left(\frac{1}{\sqrt{2}}\right) \) is well known:
\[
E\left(\frac{1}{\sqrt{2}}\right) \approx 1.350643881047676
\]
So,
\[
I \approx 2 \times 1.350643881047676 = 2.701287762095352
\]
Rounded to 10 decimal places: \( 2.7012877621 \)

**Step 6: Present in JSON Format**

```json
{"answer": "2 E\\left(\\frac{1}{\\sqrt{2}}\\right)", "numerical_answer": "2.7012877621"}
```