We want to evaluate
  I = ∫₀^(π) cos(x + cos x) dx.

Step 1. Recognize a symmetry.

Define
  f(x) = cos(x + cos x).

Perform the substitution u = π – x. Then when x = 0, u = π and when x = π, u = 0. Changing the variable (and then reordering the limits) gives

  I = ∫₀^(π) cos((π – u) + cos(π – u)) du.

Recall that
  cos(π – u) = – cos u,
so
  cos(π – u + cos(π – u)) = cos(π – u – cos u).

Now use the cosine identity:
  cos(π – y) = – cos y  (for any y).

Take y = u + cos u. Then
  cos(π – (u + cos u)) = – cos(u + cos u).

This shows that
  cos(π – u – cos u) = – cos(u + cos u).

Thus, we have
  f(π – u) = – f(u).

Step 2. Use symmetry in the integral.

Since f(π – u) = – f(u), the function is antisymmetric about π/2. Therefore,
  I = ∫₀^(π) f(x) dx = 0.

Step 3. Final Answer and Numerical Approximation.

The exact answer is 0 and numerically it is 0.0000000000 when rounded to 10 decimal places.

{"answer": "$0$", "numerical_answer": "0.0000000000"}