We wish to show that
  I = ∫₀² x^(–1/2) (2 – x)^(–1/2) (1 + 0.5 x)^(–2) · T₂(√(1 + 0.5 x)) dx
can be written in closed‐form. (Here T₂ is the Chebyshev polynomial of degree 2.) We shall explain one way of arriving at the answer.

Step 1. Rewrite the integrand in “nice” form

Recall that for the Chebyshev polynomial of the first kind the formula is
  T₂(u) = 2u² – 1.
Thus with u = √(1 + 0.5 x) one obtains
  T₂(√(1 + 0.5 x)) = 2(1 + 0.5 x) – 1 = 1 + x.
Also, (1 + 0.5 x)^(–1–1) means (1 + 0.5 x)^(–2). Therefore the integrand becomes
  x^(–½) (2 – x)^(–½) (1 + 0.5 x)^(–2) (1 + x).
In other words,
  I = ∫₀² x^(–½) (2 – x)^(–½) (1 + x) (1 + 0.5 x)^(–2) dx.

Step 2. Make a trigonometric substitution

A standard substitution for the factors x^(–½) and (2 – x)^(–½) is to set
  x = 2 sin²θ,  0 ≤ θ ≤ π/2.
Then
  dx = 4 sinθ cosθ dθ,
and
  x^(–½) = 1/√(2 sin²θ) = 1/(√2 sinθ),
  (2 – x)^(–½) = [2 – 2 sin²θ]^(–½) = 1/(√(2 cos²θ)) = 1/(√2 cosθ).
Thus the product
  x^(–½)(2 – x)^(–½) dx = (1/(√2 sinθ)) (1/(√2 cosθ)) (4 sinθ cosθ dθ)
             = [4/(2)] dθ = 2 dθ.

Next, express the remaining factors in terms of θ. We have
  1 + x = 1 + 2 sin²θ.
Also,
  1 + 0.5 x = 1 + 0.5 (2 sin²θ) = 1 + sin²θ,
so that (1 + 0.5 x)^(–2) = (1 + sin²θ)^(–2).

Thus the integral becomes
  I = 2∫₀^(π/2) (1 + 2 sin²θ)/(1 + sin²θ)² dθ.

Step 3. Change of variable

It is often advantageous to remove “extra” constants. We now write
  I = 2∫₀^(π/2) (1 + 2 sin²θ)/(1 + sin²θ)² dθ.
An alternate substitution (whose details we now describe) is to set
  u = 1 + 0.5 x.
A short calculation shows that a change of variable reduces the original integral to
  I = ∫₀¹ [2v + 1/(v + 1)²] v^(–½)(1 – v)^(–½) dv,
with v = u – 1. In our case one may show (by writing 2v + 1 = 2(v + 1) – 1) that
  (2v + 1)/(v + 1)² = 2/(v + 1) – 1/(v + 1)².
Thus
  I = 2I_A – I_B,
where
  I_A = ∫₀¹ v^(–½)(1 – v)^(–½)/(v + 1) dv  and  I_B = ∫₀¹ v^(–½)(1 – v)^(–½)/(v + 1)² dv.
These integrals can be evaluated by a standard trick. In fact, using the substitution v = sin²θ one shows that
  I_A = (π)/√2  and  I_B = (3π)/(4√2).
Thus
  I = 2(π/√2) – 3π/(4√2) = (8π – 3π)/(4√2) = (5π)/(4√2).

An independent evaluation (via the substitution x = 2 sin²θ explained earlier) leads to the same answer.

Step 4. The final answer

The final result is therefore
  I = (5π)/(4√2).

A numerical approximation is now computed:
  (5π)/(4√2) = (5 × 3.141592653589793)/(4 × 1.414213562373095) ≈ 2.7773889110.

Below is the final answer in the required JSON format.

{"answer": "$\\frac{5\\pi}{4\\sqrt{2}}$", "numerical_answer": "2.7773889110"}