Let's solve the integral:
\[
I = \int_0^{2\pi} \left|1 + 2\sin x \right| dx
\]

**Step 1: Find where the expression inside the absolute value changes sign**

Set \(1 + 2\sin x = 0\):

\[
2\sin x = -1 \implies \sin x = -\frac{1}{2}
\]

The solutions in \( [0, 2\pi] \) are:
\[
x_1 = \arcsin\left(-\frac{1}{2}\right) = \frac{7\pi}{6}
\]
\[
x_2 = \pi - \arcsin\left(-\frac{1}{2}\right) = \pi + \frac{\pi}{6} = \frac{4\pi}{3}
\]

**Verify:**

- \(\sin\left(\frac{7\pi}{6}\right) = -\frac{1}{2}\)
- \(\sin\left(\frac{11\pi}{6}\right) = -\frac{1}{2}\)

So the relevant points are \(x_1 = \frac{7\pi}{6}\), \(x_2 = \frac{11\pi}{6}\).

Check the sign of \(1+2\sin x\) in the intervals:

- For \(x\in[0, \frac{7\pi}{6})\): Let's try \(x=0\), \(\sin 0=0 \implies 1+0=1>0\).
- For \(x \in (\frac{7\pi}{6}, \frac{11\pi}{6})\): Try \(x= \pi\), \(\sin \pi = 0 \implies 1+0=1>0\)—wait, something's wrong.

Let's be careful: \(1+2\sin x=0\) at \(x_1, x_2\), what about between \(x_1\) and \(x_2\)?

Let’s try \(x = 3\pi/2\), \(\sin(3\pi/2) = -1\), so \(1 - 2 = -1 < 0\), so negative in that interval.

- \([0, \frac{7\pi}{6})\): Test \(x=0\), positive.
- \((\frac{7\pi}{6}, \frac{11\pi}{6})\): Test \(x= 3\pi/2\), negative.
- \((\frac{11\pi}{6}, 2\pi]\): Test \(x=2\pi\), \(\sin(2\pi)=0\), so positive.

Thus, the absolute value breaks as follows:
\[
I = \int_0^{\frac{7\pi}{6}} (1+2\sin x)\,dx + \int_{\frac{7\pi}{6}}^{\frac{11\pi}{6}} -(1+2\sin x)\,dx + \int_{\frac{11\pi}{6}}^{2\pi} (1+2\sin x)\,dx
\]

Let's write:
\[
I = \int_0^{\frac{7\pi}{6}} (1+2\sin x)\,dx - \int_{\frac{7\pi}{6}}^{\frac{11\pi}{6}} (1+2\sin x)\,dx + \int_{\frac{11\pi}{6}}^{2\pi} (1+2\sin x)\,dx
\]

Combine the positive intervals:
\[
I = \int_0^{\frac{7\pi}{6}} (1+2\sin x)\,dx + \int_{\frac{11\pi}{6}}^{2\pi} (1+2\sin x)\,dx - \int_{\frac{7\pi}{6}}^{\frac{11\pi}{6}} (1+2\sin x)\,dx
\]

Alternatively, add up the three integrals:

**Step 2: Evaluate each part**

The indefinite integral:
\[
\int (1+2\sin x)\,dx = x - 2\cos x + C
\]

So,
\[
I = [x-2\cos x]_0^{\frac{7\pi}{6}} 
\]
\vspace{-2mm}
\[
- [x-2\cos x]_{\frac{7\pi}{6}}^{\frac{11\pi}{6}} 
\]
\vspace{-2mm}
\[
+ [x-2\cos x]_{\frac{11\pi}{6}}^{2\pi}
\]

Compute each:

**A.** \( A_1 = [x-2\cos x]_0^{\frac{7\pi}{6}} = \frac{7\pi}{6} - 2\cos\left(\frac{7\pi}{6}\right) - [0 - 2\cos(0)] \)

Recall:
- \(\cos(0) = 1\)
- \(\cos\left(\frac{7\pi}{6}\right) = -\cos\left(\frac{\pi}{6}\right) = -\frac{\sqrt{3}}{2}\)

So,
\[
A_1 = \frac{7\pi}{6} - 2(-\frac{\sqrt{3}}{2}) - (0 - 2(1)) = \frac{7\pi}{6} + \sqrt{3} + 2
\]

**B.** \( A_2 = -\left( [x-2\cos x]_{\frac{7\pi}{6}}^{\frac{11\pi}{6}} \right) = -\left( (\frac{11\pi}{6} - 2\cos(\frac{11\pi}{6})) - (\frac{7\pi}{6} - 2\cos(\frac{7\pi}{6})) \right) \)

\[
\cos\left(\frac{11\pi}{6}\right) = \cos\left(2\pi - \frac{\pi}{6}\right) = \cos\left(\frac{\pi}{6}\right) = \frac{\sqrt{3}}{2}
\]
\[
\cos\left(\frac{7\pi}{6}\right) = -\frac{\sqrt{3}}{2}
\]

So,
\[
A_2 = -\left( \frac{11\pi}{6} - 2(\frac{\sqrt{3}}{2}) - [\frac{7\pi}{6} - 2(-\frac{\sqrt{3}}{2})] \right)
\]
\[
= -\left( \frac{11\pi}{6} - \sqrt{3} - \frac{7\pi}{6} - \sqrt{3} \right)
\]
\[
= -\left( \frac{11\pi}{6} - \frac{7\pi}{6} - \sqrt{3} - \sqrt{3} \right)
= -\left( \frac{4\pi}{6} - 2\sqrt{3} \right)
= -\left( \frac{2\pi}{3} - 2\sqrt{3} \right)
= -\frac{2\pi}{3} + 2\sqrt{3}
\]

**C.** 
\(
A_3 = [x-2\cos x]_{\frac{11\pi}{6}}^{2\pi} = 2\pi - 2\cos(2\pi) - [\frac{11\pi}{6} - 2\cos(\frac{11\pi}{6})]
\)

\[
\cos(2\pi) = 1
\]
\[
\cos\left(\frac{11\pi}{6}\right) = \frac{\sqrt{3}}{2}
\]

\[
A_3 = 2\pi - 2(1) - [\frac{11\pi}{6} - 2(\frac{\sqrt{3}}{2})]
\]
\[
= 2\pi - 2 - \frac{11\pi}{6} + \sqrt{3}
\]

Combine all terms:
\[
I = (A_1) + (A_2) + (A_3)
\]

Let's add them up:

First, sum the \(\pi\) terms:

From above:
- \(A_1: \frac{7\pi}{6}\)
- \(A_2: -\frac{2\pi}{3}\) (note: negative)
- \(A_3: 2\pi - \frac{11\pi}{6}\)

Total:
\[
\frac{7\pi}{6} - \frac{2\pi}{3} + 2\pi - \frac{11\pi}{6}
\]

Express all over 6:

- \(\frac{7\pi}{6}\)
- \(-\frac{2\pi}{3} = -\frac{4\pi}{6}\)
- \(2\pi = \frac{12\pi}{6}\)
- \(-\frac{11\pi}{6}\)

Sum:
\[
\left( \frac{7\pi}{6} - \frac{4\pi}{6} + \frac{12\pi}{6} - \frac{11\pi}{6} \right) = \frac{(7 - 4 + 12 - 11)\pi}{6} = \frac{4\pi}{6} = \frac{2\pi}{3}
\]

Now, the constants:

- \(A_1: + \sqrt{3} + 2\)
- \(A_2: + 2\sqrt{3}\)
- \(A_3: + \sqrt{3} - 2\)

Sum the constant parts:
\[
(\sqrt{3} + 2) + 2\sqrt{3} + (\sqrt{3} - 2) = (\sqrt{3} + 2\sqrt{3} + \sqrt{3}) + (2 - 2)
= (4\sqrt{3}) + 0 = 4\sqrt{3}
\]

So the exact value is:
\[
I = \frac{2\pi}{3} + 4\sqrt{3}
\]

**Step 3: Numerical approximation**

\[
\frac{2\pi}{3} \approx \frac{2 \times 3.1415926536}{3} = \frac{6.2831853072}{3} = 2.0943951024
\]
\[
4\sqrt{3} \approx 4 \times 1.7320508076 = 6.9282032304
\]

Sum:
\[
I \approx 2.0943951024 + 6.9282032304 = 9.0225983328
\]

**Final answer in JSON, as requested:**

```json
{"answer": "\\frac{2\\pi}{3} + 4\\sqrt{3}", "numerical_answer": "9.0225983328"}
```