<think>
Okay, let's tackle this integral ∫ from -4 to 4 of e^|x| times the fractional part of x, which is denoted as {x} dx. Hmm, first, I need to recall what the fractional part function does. The fractional part {x} is x minus the floor of x, right? So for any real number x, {x} = x - ⌊x⌋. That means {x} is always between 0 (inclusive) and 1 (exclusive). 

Now, the integral is from -4 to 4. Since the integrand involves |x| and {x}, I should consider the behavior of these functions over the interval. Let me break down the integral into parts where the functions |x| and {x} have different expressions. 

First, let's think about the absolute value function |x|. For x ≥ 0, |x| = x, and for x < 0, |x| = -x. So the integrand e^|x| will be e^x for non-negative x and e^{-x} for negative x. 

Next, the fractional part {x}. For positive x, {x} is just x minus the integer part. For example, between 0 and 1, {x} = x; between 1 and 2, {x} = x - 1, and so on. For negative x, the fractional part is a bit trickier. Since ⌊x⌋ for x in [-1, 0) is -1, so {x} = x - (-1) = x + 1. Similarly, for x in [-2, -1), {x} = x - (-2) = x + 2, etc. 

So, the interval from -4 to 4 can be divided into integer segments where both |x| and {x} can be expressed without the absolute value or floor functions. Let's list these intervals:

Negative side:
- From -4 to -3: here, x is in [-4, -3), so ⌊x⌋ = -4, so {x} = x - (-4) = x + 4. And |x| = -x.
- From -3 to -2: {x} = x + 3, |x| = -x.
- From -2 to -1: {x} = x + 2, |x| = -x.
- From -1 to 0: {x} = x + 1, |x| = -x.

Positive side:
- From 0 to 1: {x} = x, |x| = x.
- From 1 to 2: {x} = x - 1, |x| = x.
- From 2 to 3: {x} = x - 2, |x| = x.
- From 3 to 4: {x} = x - 3, |x| = x.

So the integral can be split into 8 intervals: four on the negative side and four on the positive side. Let's write each integral as a sum of these intervals.

Let me denote the integral as I = ∫_{-4}^4 e^{|x|} {x} dx = sum_{k=-4}^{-1} ∫_{k}^{k+1} e^{-x} (x - k) dx + sum_{k=0}^{3} ∫_{k}^{k+1} e^{x} (x - k) dx.

Wait, actually, for the negative side, each interval from k to k+1 where k is -4, -3, -2, -1. For each of these, {x} = x - k (since k is negative, so floor(x) is k, so {x} = x - k). But in the negative intervals, for example, from -4 to -3, floor(x) is -4, so {x} = x - (-4) = x +4. Similarly, from -3 to -2, {x} = x +3, etc. So in general, for x in [n, n+1) where n is an integer, {x} = x - n. But when n is negative, like n = -4, then {x} = x - (-4) = x +4. So, for each interval [n, n+1), {x} = x - n. So the expression for {x} is the same regardless of n being positive or negative. However, the absolute value |x| is different. For x in [n, n+1) where n < 0, |x| = -x. For n >=0, |x| = x.

Therefore, the integral can be written as the sum over n from -4 to 3 of ∫_{n}^{n+1} e^{|x|} (x - n) dx.

But since the integral from -4 to 4 is split into intervals between each integer from -4 up to 4. So n ranges from -4 to 3. Each integral is over [n, n+1). So let's split the integral into 8 parts:

1. From -4 to -3: n = -4
2. From -3 to -2: n = -3
3. From -2 to -1: n = -2
4. From -1 to 0: n = -1
5. From 0 to 1: n = 0
6. From 1 to 2: n = 1
7. From 2 to 3: n = 2
8. From 3 to 4: n = 3

For each of these, we can compute the integral ∫_{n}^{n+1} e^{|x|} (x - n) dx.

Now, let's handle each interval:

For n from -4 to -1 (negative intervals):

In these intervals, x is in [n, n+1), which is negative. So |x| = -x. Therefore, the integrand becomes e^{-x} (x - n). So the integral for each such n is ∫_{n}^{n+1} e^{-x} (x - n) dx.

For n from 0 to 3 (positive intervals):

Here, x is non-negative, so |x| = x. The integrand is e^{x} (x - n). So the integral is ∫_{n}^{n+1} e^{x} (x - n) dx.

Therefore, the total integral I is the sum of the integrals over the negative intervals and the positive intervals.

Let me compute each integral separately.

First, let's handle the negative intervals (n = -4, -3, -2, -1):

For each n from -4 to -1, compute I_n = ∫_{n}^{n+1} e^{-x} (x - n) dx.

Let’s make a substitution to simplify. Let t = x - n. Then when x = n, t = 0; when x = n+1, t = 1. Then dx = dt. So the integral becomes ∫_{0}^{1} e^{-(n + t)} (t) dt = e^{-n} ∫_{0}^{1} e^{-t} t dt.

Because e^{-x} = e^{-(n + t)} = e^{-n} e^{-t}.

So I_n = e^{-n} ∫_{0}^{1} t e^{-t} dt.

The integral ∫ t e^{-t} dt from 0 to 1 is a standard integral. Let's compute it:

∫ t e^{-t} dt. Integration by parts: let u = t, dv = e^{-t} dt. Then du = dt, v = -e^{-t}.

So uv - ∫ v du = -t e^{-t} + ∫ e^{-t} dt = -t e^{-t} - e^{-t} + C.

Evaluated from 0 to 1:

[-1 e^{-1} - e^{-1}] - [0 - e^{0}] = (-e^{-1} - e^{-1}) - (-1) = (-2 e^{-1}) + 1 = 1 - 2/e.

Therefore, ∫_{0}^{1} t e^{-t} dt = 1 - 2/e.

Therefore, each I_n for n from -4 to -1 is e^{-n} (1 - 2/e).

But wait, n is negative here. For example, n = -4, then e^{-n} = e^{4}; for n = -3, e^{-n} = e^{3}, etc.

So the sum over the negative intervals (n = -4, -3, -2, -1):

Sum_{n=-4}^{-1} I_n = (1 - 2/e) [e^{4} + e^{3} + e^{2} + e^{1}].

Similarly, for the positive intervals (n = 0, 1, 2, 3):

Compute I_n = ∫_{n}^{n+1} e^{x} (x - n) dx.

Again, let’s substitute t = x - n. Then x = n, t=0; x = n+1, t=1. So dx = dt, and the integral becomes ∫_{0}^{1} e^{n + t} t dt = e^{n} ∫_{0}^{1} t e^{t} dt.

Compute ∫ t e^{t} dt from 0 to 1. Again, integration by parts. Let u = t, dv = e^{t} dt. Then du = dt, v = e^{t}.

uv - ∫ v du = t e^{t} - ∫ e^{t} dt = t e^{t} - e^{t} + C.

Evaluated from 0 to 1:

[1 e^{1} - e^{1}] - [0 - e^{0}] = (e - e) - (-1) = 0 + 1 = 1.

Therefore, ∫_{0}^{1} t e^{t} dt = 1.

Therefore, each I_n for n = 0,1,2,3 is e^{n} * 1 = e^{n}.

So the sum over the positive intervals is Sum_{n=0}^{3} e^{n} = e^{0} + e^{1} + e^{2} + e^{3} = 1 + e + e² + e³.

Therefore, the total integral I is:

I = (1 - 2/e)(e⁴ + e³ + e² + e) + (1 + e + e² + e³).

Let me compute this expression step by step.

First, compute the sum of e⁴ + e³ + e² + e ). Let's factor out e:

e( e³ + e² + e + 1 ). Wait, actually, e⁴ + e³ + e² + e = e(e³ + e² + e + 1) = e*(sum from k=0 to 3 e^k). Wait, no, e³ + e² + e + 1 is sum from k=0 to 3 of e^k. So e⁴ + e³ + e² + e = e*(sum_{k=0}^3 e^k). But sum_{k=0}^3 e^k = (e⁴ - 1)/(e - 1). Wait, sum_{k=0}^n e^k = (e^{n+1} - 1)/(e - 1). So for n=3, sum is (e^4 -1)/(e -1). Therefore, e*(sum) = e*(e^4 -1)/(e -1). But maybe it's better to compute numerically later.

But let's proceed step by step.

First, compute (1 - 2/e) multiplied by (e⁴ + e³ + e² + e):

Let’s compute (1 - 2/e) * (e⁴ + e³ + e² + e) = (1 - 2/e) * e*(e³ + e² + e + 1) = e*(1 - 2/e)*(e³ + e² + e +1 )

But maybe expanding directly:

(1 - 2/e)(e⁴ + e³ + e² + e) = e⁴(1 - 2/e) + e³(1 - 2/e) + e²(1 - 2/e) + e(1 - 2/e)

= e⁴ - 2e³ + e³ - 2e² + e² - 2e + e - 2

Wait, let's compute each term:

First term: e⁴*(1 - 2/e) = e⁴ - 2e³

Second term: e³*(1 - 2/e) = e³ - 2e²

Third term: e²*(1 - 2/e) = e² - 2e

Fourth term: e*(1 - 2/e) = e - 2

So adding all these together:

(e⁴ - 2e³) + (e³ - 2e²) + (e² - 2e) + (e - 2) =

Combine like terms:

e⁴ -2e³ + e³ = e⁴ - e³

Then -2e² + e² = -e²

Then -2e + e = -e

Then -2.

So overall: e⁴ - e³ - e² - e - 2.

Wait, let me check:

First term: e⁴ -2e³

Second term: + e³ -2e² → total e⁴ - e³ -2e²

Third term: + e² -2e → total e⁴ - e³ - e² -2e

Fourth term: + e -2 → total e⁴ - e³ - e² - e -2.

Yes, that's correct.

Then, the other part of the integral is the sum of the positive intervals: 1 + e + e² + e³.

So total integral I = (e⁴ - e³ - e² - e -2) + (1 + e + e² + e³) = e⁴ - e³ - e² - e -2 +1 + e + e² + e³

Simplify term by term:

e⁴ remains.

- e³ + e³ = 0

- e² + e² = 0

- e + e = 0

-2 +1 = -1

So total integral I = e⁴ -1.

Wait, that's surprising. All the middle terms cancel out, leaving e⁴ -1 -1? Wait, no:

Wait, let's recheck:

Original expression:

(e⁴ - e³ - e² - e -2) + (1 + e + e² + e³)

Combine:

e⁴ + (-e³ + e³) + (-e² + e²) + (-e + e) + (-2 +1)

Which is e⁴ + 0 +0 +0 + (-1) = e⁴ -1.

So the integral simplifies to e⁴ -1.

Wait, that's a very clean result. So the integral from -4 to 4 of e^{|x|} {x} dx equals e⁴ -1.

But let me verify this because it's surprising. Let me check the steps again.

First, the negative intervals contributed (1 - 2/e)(e⁴ + e³ + e² + e) which expanded to e⁴ - e³ - e² - e -2.

Then the positive intervals contributed 1 + e + e² + e³.

Adding them together:

e⁴ - e³ - e² - e -2 +1 + e + e² + e³

= e⁴ + (-e³ + e³) + (-e² + e²) + (-e + e) + (-2 +1)

= e⁴ + 0 +0 +0 -1 = e⁴ -1.

Yes, that's correct. So the integral is e⁴ -1. That's the exact answer.

But wait, is this possible? Let me think. The integral over the entire interval from -4 to 4 of e^{|x|} {x} dx equals e⁴ -1. Let me check with a numerical approximation.

Compute e⁴: e^4 ≈ 54.5981500331

So e⁴ -1 ≈ 54.5981500331 -1 ≈ 53.5981500331.

But let's compute the integral numerically step by step to check.

Alternatively, let's compute the sum of the negative intervals and positive intervals.

First, compute the negative intervals:

Sum_{n=-4}^{-1} I_n = (1 - 2/e)(e^4 + e^3 + e^2 + e)

Compute 1 - 2/e ≈ 1 - 2/2.718281828459045 ≈ 1 - 0.7357588823 ≈ 0.2642411177.

Then e^4 + e^3 + e^2 + e ≈ 54.59815 + 20.0855369 + 7.389056 + 2.718281 ≈ 54.59815 +20.0855369=74.6836869 +7.389056=82.0727429 +2.718281≈84.7910239.

Multiply by 0.2642411177: 84.7910239 * 0.2642411177 ≈ Let's compute:

84.7910239 * 0.2 = 16.95820478

84.7910239 * 0.06 = 5.087461434

84.7910239 * 0.0042411177 ≈ approx 84.7910239 *0.004=0.339164, and 84.7910239*0.0002411177≈0.02044. So total ≈0.339164+0.02044≈0.3596.

Adding all: 16.9582 +5.08746 +0.3596 ≈22.40526.

So the negative intervals contribute approximately 22.40526.

The positive intervals sum to 1 + e + e² + e³ ≈1 +2.71828 +7.38906 +20.085537≈1+2.71828=3.71828+7.38906=11.10734+20.085537≈31.192877.

So total integral ≈22.40526 +31.192877≈53.598137, which is approximately 53.59815, which is e^4 -1 ≈54.59815 -1≈53.59815. So this matches. Therefore, the analytical result e⁴ -1 is correct.

Therefore, the exact answer is e⁴ -1, and the numerical approximation is approximately 53.5981500331, which rounds to 53.5981500331. Rounded to 10 decimal places, that's 53.5981500331 → 53.5981500331. Wait, but let me check with more precise calculation.

But e is approximately 2.718281828459045, so e^4 is e squared squared: e^2 ≈7.38905609893, then e^4 = (e^2)^2 ≈ (7.38905609893)^2 ≈54.598150033144236. Therefore, e^4 -1 ≈53.598150033144236. Rounded to 10 decimal places, that's 53.5981500331.

So the exact answer is e^4 -1, and the numerical answer is approximately 53.5981500331.

Therefore, the final answer is {"answer": "e^4 - 1", "numerical_answer": 53.5981500331}.

But let me check once more if there's any mistake in the analytical steps. The key step was realizing that the sum over the negative intervals and positive intervals simplifies to e^4 -1. Since the intermediate terms canceled out, leading to e^4 -1. Given that the numerical approximation matches, this seems correct.

Another way to think about it: the integral over each interval [n, n+1) for n from -4 to 3, the sum of all these integrals simplifies to e^4 -1. It's a bit surprising, but the math checks out. So I think this is correct.
</think>

{"answer": "e^4 - 1", "numerical_answer": "53.5981500331"}