# Evaluation of $\int\limits_0^2 x^{1/2}(2-x)^{-1/2}\cosh\left(\sqrt{x(2-x)}\right)dx$

## Step 1: Analyze the integral

Let's examine the integral:
$$\int\limits_0^2 x^{1/2}(2-x)^{-1/2}\cosh\left(\sqrt{x(2-x)}\right)dx$$

This looks quite complex. Let's try a substitution to simplify it.

## Step 2: Substitution

Let's set $u = \sqrt{x(2-x)}$. We need to find $du$ and express $dx$ in terms of $du$.

Note that $u^2 = x(2-x) = 2x - x^2$

Taking the derivative:
$2u \cdot du = 2 - 2x$
$du = \frac{1-x}{u}$

Also, we can rewrite $x$ in terms of $u$ by solving the quadratic equation:
$x^2 - 2x + u^2 = 0$

Using the quadratic formula:
$x = 1 \pm \sqrt{1-u^2}$

Since $x$ ranges from 0 to 2, we'll use $x = 1 - \sqrt{1-u^2}$ when $x < 1$ and $x = 1 + \sqrt{1-u^2}$ when $x > 1$.

## Step 3: Let's try a different approach

The substitution is getting complicated. Let's try a different approach.

Notice that we can rewrite the integral using the substitution $x = 2\sin^2 t$ for $0 \leq t \leq \pi/2$.

With this substitution:
- $dx = 4\sin t \cos t \, dt$
- $2-x = 2-2\sin^2 t = 2\cos^2 t$
- $\sqrt{x(2-x)} = \sqrt{2\sin^2 t \cdot 2\cos^2 t} = 2\sin t \cos t$

## Step 4: Applying the substitution

With $x = 2\sin^2 t$:
- $x^{1/2} = \sqrt{2} \cdot \sin t$
- $(2-x)^{-1/2} = (2\cos^2 t)^{-1/2} = \frac{1}{\sqrt{2} \cdot \cos t}$
- $\cosh\left(\sqrt{x(2-x)}\right) = \cosh(2\sin t \cos t)$
- $dx = 4\sin t \cos t \, dt$

Substituting these into the integral:

$$\int\limits_0^2 x^{1/2}(2-x)^{-1/2}\cosh\left(\sqrt{x(2-x)}\right)dx = \int\limits_0^{\pi/2} \sqrt{2} \sin t \cdot \frac{1}{\sqrt{2} \cos t} \cdot \cosh(2\sin t \cos t) \cdot 4\sin t \cos t \, dt$$

Simplifying:
$$\int\limits_0^{\pi/2} 4\sin^2 t \cdot \cosh(2\sin t \cos t) \, dt$$

## Step 5: Further simplification

Let's use the identity $\sin^2 t = \frac{1-\cos(2t)}{2}$:

$$\int\limits_0^{\pi/2} 4 \cdot \frac{1-\cos(2t)}{2} \cdot \cosh(2\sin t \cos t) \, dt$$

$$\int\limits_0^{\pi/2} 2(1-\cos(2t)) \cdot \cosh(2\sin t \cos t) \, dt$$

We also know that $\sin t \cos t = \frac{\sin(2t)}{2}$, so:

$$\int\limits_0^{\pi/2} 2(1-\cos(2t)) \cdot \cosh(\sin(2t)) \, dt$$

## Step 6: Another substitution

Let's set $v = 2t$, which gives $dv = 2dt$ and changes the limits to $0$ and $\pi$:

$$\int\limits_0^{\pi} (1-\cos v) \cdot \cosh\left(\sin v\right) \, dv$$

This integral can be split:

$$\int\limits_0^{\pi} \cosh\left(\sin v\right) \, dv - \int\limits_0^{\pi} \cos v \cdot \cosh\left(\sin v\right) \, dv$$

## Step 7: Evaluating the first integral

For $\int\limits_0^{\pi} \cosh\left(\sin v\right) \, dv$, we can use the fact that $\sin v$ is antisymmetric about $v = \pi/2$. Since $\cosh$ is an even function, $\cosh(\sin v)$ is symmetric about $v = \pi/2$.

Therefore:
$$\int\limits_0^{\pi} \cosh\left(\sin v\right) \, dv = 2\int\limits_0^{\pi/2} \cosh\left(\sin v\right) \, dv$$

## Step 8: Evaluating the second integral

For the second integral $\int\limits_0^{\pi} \cos v \cdot \cosh\left(\sin v\right) \, dv$, we can use the fact that $\cosh(x)$ is the derivative of $\sinh(x)$.

Let $u = \sin v$, then $du = \cos v \, dv$:

$$\int \cos v \cdot \cosh\left(\sin v\right) \, dv = \int \cosh(u) \, du = \sinh(u) + C = \sinh(\sin v) + C$$

Evaluating from $0$ to $\pi$:
$$\left[ \sinh(\sin v) \right]_0^{\pi} = \sinh(\sin \pi) - \sinh(\sin 0) = \sinh(0) - \sinh(0) = 0$$

## Step 9: Bringing it all together

We have:
$$\int\limits_0^2 x^{1/2}(2-x)^{-1/2}\cosh\left(\sqrt{x(2-x)}\right)dx = \int\limits_0^{\pi} \cosh\left(\sin v\right) \, dv = 2\int\limits_0^{\pi/2} \cosh\left(\sin v\right) \, dv$$

This integral equals $2\pi I_0(1)$, where $I_0$ is the modified Bessel function of the first kind of order 0. 

Therefore, the exact answer is:
$$\int\limits_0^2 x^{1/2}(2-x)^{-1/2}\cosh\left(\sqrt{x(2-x)}\right)dx = 2\pi I_0(1)$$

## Step 10: Numerical approximation

The value of $I_0(1)$ is approximately 1.2660658777, so:
$2\pi I_0(1) \approx 2\pi \cdot 1.2660658777 \approx 7.9577471546$

{"answer": "2\\pi I_0(1)", "numerical_answer": "7.9577471546"}