We will show that
  I = ∫₀² [1/x]·√(4–x²)·arctan(x) dx
can be written in closed‐form. One acceptable answer is

  I = π·ln(2+√5) – (π/2)(√5 – 1).

Below we describe one route to this answer.

Step 1. Write the given integral as
  I = ∫₀² x^(–1)√(4–x²)·arctan(x) dx.

Step 2. Express arctan(x) by an integral representation. One may use
  arctan(x) = ∫₀¹ [x/(1+t²x²)] dt  (for x ≥ 0).
Then, by Fubini’s theorem we may interchange the order of integration:
  I = ∫₀² [1/x]√(4–x²) [∫₀¹ x/(1+t²x²) dt] dx
   = ∫₀¹ [∫₀² √(4–x²)/(1+t²x²) dx] dt.
Define
  J(t) = ∫₀² √(4–x²)/(1+t²x²) dx.

Step 3. Make the substitution x = 2 sinθ (so that when x=0, θ=0, and when x=2, θ=π/2). Then
  dx = 2 cosθ dθ  and  √(4–x²) = 2 cosθ.
Thus
  J(t) = ∫₀^(π/2) [2 cosθ/(1+4t² sin²θ)] · [2 cosθ dθ]
     = 4∫₀^(π/2) [cos²θ/(1+4t² sin²θ)] dθ.

Now write cos²θ = 1 – sin²θ so that
  J(t) = 4 [∫₀^(π/2) 1/(1+4t² sin²θ)dθ – ∫₀^(π/2) sin²θ/(1+4t² sin²θ)dθ].

There are standard formulas for these integrals:
  ∫₀^(π/2) dθ/(1+M sin²θ) = π/(2√(1+M)),
  ∫₀^(π/2) (sin²θ dθ)/(1+M sin²θ) = (π/(2M))(1 – 1/√(1+M)).
In our case M = 4t². Hence we obtain
  J(t) = 4 [π/(2√(1+4t²)) – π/(2·4t²)(1 – 1/√(1+4t²))]
   = 2π/√(1+4t²) – (π/(2t²)) (1 – 1/√(1+4t²)).

Step 4. Thus the original integral becomes
  I = ∫₀¹ J(t) dt
   = 2π∫₀¹ dt/√(1+4t²) – (π/2)∫₀¹ (1 – 1/√(1+4t²))/t² dt.
Call the two t–integrals A and B so that
  I = 2π A – (π/2) B.

The first integral is elementary:
  A = ∫₀¹ dt/√(1+4t²) = (1/2)·asinh(2) = (1/2) ln(2+√5).

Now the second integral can be written as
  B = ∫₀¹ [1/t² – 1/(t²√(1+4t²))] dt.
One may verify by differentiating
  F(t) = (√(1+4t²) – 1)/t,
that
  F′(t) = [√(1+4t²) – 1]/(t²√(1+4t²))
which shows that an antiderivative for the integrand in B is F(t). In particular,
  B = F(1) – limₜ→0 F(t).
A short series expansion shows that limₜ→0 F(t) = 0 so that
  B = (√(1+4·1²) – 1) = (√5 – 1).

Thus we have
  I = 2π·(1/2) ln(2+√5) – (π/2)(√5–1)
   = π ln(2+√5) – (π/2)(√5 – 1).

Step 5. Numerical approximation

Now, using:
  √5 ≈ 2.2360679775  and  ln(2+√5) = ln(4.2360679775) ≈ 1.4436354750,
we get
  π ln(2+√5) ≈ 3.1415926536 × 1.4436354750 ≈ 4.5349064250,
  (π/2)(√5 – 1) ≈ 1.5707963268 × 1.2360679775 ≈ 1.9416110387.
Thus,
  I ≈ 4.5349064250 – 1.9416110387 ≈ 2.5932953863.

The final answer is given below in the required JSON format.

{"answer": "\\pi \\ln(2+\\sqrt{5}) - \\frac{\\pi}{2}(\\sqrt{5}-1)", "numerical_answer": "2.5932953863"}