

To solve the definite integral \(\int_{-1}^1 x^2 \cdot \sqrt[3]{x^3 + 1} \, dx\), we use the substitution method.

### Step 1: Substitution
Let \( u = x^3 + 1 \). Then, the differential \( du \) is:
\[
du = 3x^2 \, dx \implies x^2 \, dx = \frac{1}{3} du
\]

### Step 2: Adjust Limits of Integration
When \( x = -1 \):
\[
u = (-1)^3 + 1 = 0
\]
When \( x = 1 \):
\[
u = (1)^3 + 1 = 2
\]
Thus, the integral transforms from \( x \in [-1, 1] \) to \( u \in [0, 2] \).

### Step 3: Rewrite the Integral
Substituting \( u \) and \( du \) into the integral:
\[
\int_{-1}^1 x^2 \cdot \sqrt[3]{x^3 + 1} \, dx = \int_{0}^{2} \sqrt[3]{u} \cdot \frac{1}{3} du = \frac{1}{3} \int_{0}^{2} u^{1/3} \, du
\]

### Step 4: Integrate
The integral of \( u^{1/3} \) with respect to \( u \) is:
\[
\int u^{1/3} \, du = \frac{u^{4/3}}{4/3} + C = \frac{3}{4} u^{4/3} + C
\]
Thus,
\[
\frac{1}{3} \int_{0}^{2} u^{1/3} \, du = \frac{1}{3} \left[ \frac{3}{4} u^{4/3} \right]_{0}^{2} = \frac{1}{4} \left[ u^{4/3} \right]_{0}^{2}
\]

### Step 5: Evaluate the Definite Integral
Substituting the limits \( u = 0 \) and \( u = 2 \):
\[
\frac{1}{4} \left( 2^{4/3} - 0^{4/3} \right) = \frac{1}{4} \cdot 2^{4/3}
\]
Simplify \( 2^{4/3} = 2 \cdot 2^{1/3} \), so:
\[
\frac{1}{4} \cdot 2 \cdot 2^{1/3} = \frac{1}{2} \cdot 2^{1/3} = \frac{\sqrt[3]{2}}{2}
\]

### Numerical Approximation
The cube root of 2 is approximately \( \sqrt[3]{2} \approx 1.259921049894873 \). Dividing by 2 gives:
\[
\frac{\sqrt[3]{2}}{2} \approx 0.6299605249474365
\]
Rounded to 10 decimal places, this is \( 0.6299605249 \).

{"answer": "\\frac{\\sqrt[3]{2}}{2}", "numerical_answer": "0.6299605249"}