Let's tackle the integral:

\[
I = \int_0^{2\pi} \left\lfloor 2023\sin(x) \right\rfloor dx
\]

### 1. Understanding the Problem

We are to integrate the floor function of \(2023\sin(x)\) from \(0\) to \(2\pi\).

Key facts about \(\sin(x)\) over \(x \in [0, 2\pi]\):

- \(\sin(x)\) attains all values in \([-1, 1]\).
- Therefore, \(2023\sin(x)\) attains all values in \([-2023, 2023]\).

For each integer \(k\) in \([-2023, 2022]\), the set of \(x\) for which 
\[
k \leq 2023\sin(x) < k + 1
\]
is nonempty. For integer \(k = k_0\), the set corresponds to
\[
\sin(x) \in \left[\frac{k}{2023}, \frac{k+1}{2023}\right)
\]
But since \(\sin(x)\) only attains values in \([-1, 1]\), only those \(k\) with
\[
-2023 \leq k \leq 2022
\]
and for which this interval is a subset of \([-1, 1)\) are considered.

Let us precisely note the range of \(k\):

- When \(k = 2023\), \(\sin(x)\) would need to be at least 1, which occurs only at discrete points, so for all practical purposes, the interval for \(k=2023\) is empty.
- Thus, \(k\) ranges from \(-2023\) to \(2022\).

Let us write
\[
I = \sum_{k = -2023}^{2022} \int_{\substack{x\in[0,2\pi]\\2023\sin(x)\in[k,k+1)}} k\;dx = \sum_{k = -2023}^{2022} k \cdot |S_k|
\]
where \(S_k\) is the set of \(x\) values in \([0,2\pi]\) such that \(2023\sin(x)\in[k,k+1)\):
\[
|S_k| = \text{meas}\left\{x \in [0,2\pi] : \frac{k}{2023} \leq \sin(x) < \frac{k+1}{2023} \right\}
\]

### 2. Compute the measure \(|S_k|\)

For \(a,b \in [-1,1]\) and \(a < b\), the measure of \(x\in[0,2\pi]\) where \(\sin(x)\in[a,b)\) is:
\[
|S(a,b)| = 2\left(\arcsin(b) - \arcsin(a)\right)
\]

So for each \(k\),
\[
|S_k| = 2\left(\arcsin\left(\frac{k+1}{2023}\right) - \arcsin\left(\frac{k}{2023}\right)\right)
\]
as long as both \(\frac{k}{2023}\) and \(\frac{k+1}{2023}\) are in \([-1,1]\).

But we need to restrict to exactly those \(k\) for which the intervals are within \([-1,1)\):
- Lower bound: \(k \geq -2023\)
- Upper bound: \(k+1 < 2023 \implies k \leq 2021\) -- but really, \(\frac{k+1}{2023} < 1\), so \(k+1 < 2023 \rightarrow k \leq 2021\).

But for \(k = 2022\), \(\frac{k+1}{2023} = \frac{2023}{2023} = 1\), so \([2022/2023,1]\): that's a valid interval, but right endpoint is not included because of the strict inequality in the floor. So for the upper limit of \(k = 2022\), the interval is \([2022/2023,1)\).

No such values for \(\sin(x) = 1\) except at discrete \(x\).

So, to avoid ambiguities at endpoints, summing from \(k = -2023\) to \(2022\) is valid.

Therefore, the integral can be expressed as:
\[
I = \sum_{k=-2023}^{2022} k \cdot 2\left[\arcsin\left(\frac{k+1}{2023}\right) - \arcsin\left(\frac{k}{2023}\right)\right]
\]

### 3. Simplification

Let’s expand the sum:
\[
I = 2\sum_{k=-2023}^{2022} k \left[\arcsin\left(\frac{k+1}{2023}\right) - \arcsin\left(\frac{k}{2023}\right)\right]
\]

Let’s write:
\[
I = 2\left[\sum_{k=-2023}^{2022} k \arcsin\left(\frac{k+1}{2023}\right) - \sum_{k=-2023}^{2022} k \arcsin\left(\frac{k}{2023}\right)\right]
\]

Change index in the first sum by letting \(l = k+1\):

\[
\sum_{k=-2023}^{2022} k\arcsin\left(\frac{k+1}{2023}\right) = \sum_{l=-2022}^{2023} (l-1)\arcsin\left(\frac{l}{2023}\right)
\]
So,
\[
I = 2\left[\sum_{l=-2022}^{2023} (l-1)\arcsin\left(\frac{l}{2023}\right) - \sum_{k=-2023}^{2022} k\arcsin\left(\frac{k}{2023}\right)\right]
\]
\[
= 2\left[\sum_{l=-2022}^{2023} (l-1)\arcsin\left(\frac{l}{2023}\right) - \sum_{l=-2023}^{2022} l \arcsin\left(\frac{l}{2023}\right)\right]
\]
\[
= 2\left[\sum_{l=-2022}^{2023} (l-1)\arcsin\left(\frac{l}{2023}\right) - \sum_{l=-2022}^{2022} l \arcsin\left(\frac{l}{2023}\right) - (-2023)\arcsin\left(\frac{-2023}{2023}\right) \right]
\]
Here, when expanding \(\sum_{l=-2023}^{2022}\), the lower limit is \(l=-2023\), so pull out that term.

\[
= 2\left[ \sum_{l=-2022}^{2022} (l-1)\arcsin\left(\frac{l}{2023}\right) + (2023-1)\arcsin(1) - \sum_{l=-2022}^{2022} l\arcsin\left(\frac{l}{2023}\right) - (-2023)\arcsin(-1) \right]
\]

Wait, but \(l=2023\) appears only in the first sum, so extract it:

\[
= 2 \left\{ \sum_{l=-2022}^{2022} [(l-1)\arcsin\left(\frac{l}{2023}\right) - l\arcsin\left(\frac{l}{2023}\right)] + (2023-1)\arcsin(1) - (-2023)\arcsin(-1) + (2023) \arcsin\left(\frac{2023}{2023}\right) \right\}
\]
But \(2023\arcsin(1)\) is for \(l = 2023\), so the sum is:

- \(l = -2022\) to \(2022\): difference is \((l-1) - l = -1\)
- At \(l=2023\): \((2023-1)\arcsin(1)\)
- The vacuumed \(-2023\arcsin(-1)\) from the lower limit.

So:

\[
\sum_{l=-2022}^{2022} [(l-1) - l]\arcsin\left(\frac{l}{2023}\right) = \sum_{l=-2022}^{2022} (-1)\arcsin\left(\frac{l}{2023}\right) = -\sum_{l=-2022}^{2022} \arcsin\left(\frac{l}{2023}\right)
\]

Also, \((2023-1)\arcsin(1) = 2022\arcsin(1)\) and \(-(-2023)\arcsin(-1) = 2023\arcsin(-1)\).

Finally, the term for \(l=2023\) in the first sum is \((2023-1)\arcsin(1) = 2022\arcsin(1)\).

But perhaps the sum limits need to be checked once more. Let's match terms precisely.

Define for \(l = -2023\) to \(2023\):

- For \(k\) from \(-2023\) to \(2022\):

  - \(k\arcsin\left(\frac{k+1}{2023}\right)\) as \(l = k+1\) goes from \(-2022\) to \(2023\)

- So the net effect is:

\[
I = 2 \left[- \sum_{l=-2022}^{2022} \arcsin\left(\frac{l}{2023}\right) + 2022 \arcsin(1) + 2023 \arcsin(-1)\right]
\]

Now, \( \arcsin(1) = \frac{\pi}{2} \) and \( \arcsin(-1) = -\frac{\pi}{2} \).

So,

\[
I = 2\left[-\sum_{l=-2022}^{2022} \arcsin\left(\frac{l}{2023}\right) + 2022\cdot \frac{\pi}{2} + 2023 \cdot (-\frac{\pi}{2}) \right]
\]
\[
= 2\left[-\sum_{l=-2022}^{2022} \arcsin\left(\frac{l}{2023}\right) - \frac{\pi}{2} \right]
\]
\[
= -2\sum_{l=-2022}^{2022} \arcsin\left(\frac{l}{2023}\right) - \pi
\]

### 4. Exact Analytical Final Answer

The exact value is:

\[
\boxed{
I = -2\sum_{l=-2022}^{2022} \arcsin\left(\frac{l}{2023}\right) - \pi
}
\]

### 5. Numerical Evaluation

Let’s numerically approximate \(I\):

The sum \(\sum_{l=-2022}^{2022} \arcsin\left(\frac{l}{2023}\right)\):

There are \(4045\) terms in the sum from \(l = -2022\) to \(2022\).

The sum
\[
S = \sum_{l=-2022}^{2022} \arcsin\left(\frac{l}{2023}\right)
\]

Notice that \(\arcsin(-x) = -\arcsin(x)\), so terms cancel in pairs except for \(l = 0\), where the term is \(0\).

So,

\[
S = \sum_{l=1}^{2022} \left[ \arcsin\left( \frac{l}{2023} \right) + \arcsin\left(-\frac{l}{2023}\right) \right] + \arcsin(0)
= 0 + \sum_{l=1}^{2022} 0
\]
But that's not quite right, because \(\arcsin(-x) = -\arcsin(x)\), so

\[
S = 0 + \sum_{l=1}^{2022} ( \arcsin(\frac{l}{2023}) - \arcsin(\frac{l}{2023}) ) = 0
\]
But this would lead to zero, which cannot be.

But actually, the sum from \(l = -n\) to \(n\) of an odd function is zero. But here it's not quite an odd function because the interval is slightly asymmetric (\(l=-2022\) to \(l=2022\)), total \(4045\) terms, and \(l=0\) is zero.

Wait, but perhaps the key is to see that

\[
S = \sum_{l=-2022}^{2022} \arcsin\left( \frac{l}{2023} \right )
\]
Since for each \(l\), \( \arcsin\left( \frac{-l}{2023} \right ) = -\arcsin\left( \frac{l}{2023} \right ) \), these terms cancel for \(l \neq 0\). There are \(2022\) positive \(l\) and \(2022\) negative \(l\), and \(l=0\).

Thus,

\[
S = \arcsin(0) = 0
\]
So,

\[
I = -2 \times 0 - \pi = -\pi
\]

Wait, this is surprising! Let us double check this result.

Recall the sum cancels pairwise for negative and positive \(l\), each pair adding to zero, and the middle term is \(\arcsin(0) = 0\).

Therefore, the sum is zero. Thus,

\[
I = -\pi
\]

### 6. Numerical Approximation

\[
-\pi \approx -3.1415926536
\]

---

### 7. Output in JSON

```json
{"answer": "-\\pi", "numerical_answer": "-3.1415926536"}
```