To solve the definite integral \(\int_0^\infty \frac{\tanh(x)}{e^x} \, dx\), we will follow the steps outlined:

### Step 1: Analytical Computation

First, recall the definition of the hyperbolic tangent function:
\[
\tanh(x) = \frac{e^x - e^{-x}}{e^x + e^{-x}}
\]

We can rewrite the integrand:
\[
\frac{\tanh(x)}{e^x} = \frac{e^x - e^{-x}}{e^x (e^x + e^{-x})} = \frac{e^x - e^{-x}}{e^{2x} + 1}
\]

Thus, the integral becomes:
\[
\int_0^\infty \frac{e^x - e^{-x}}{e^{2x} + 1} \, dx
\]

We can split this into two separate integrals:
\[
\int_0^\infty \frac{e^x}{e^{2x} + 1} \, dx - \int_0^\infty \frac{e^{-x}}{e^{2x} + 1} \, dx
\]

Let's evaluate each integral separately.

#### First Integral:
\[
\int_0^\infty \frac{e^x}{e^{2x} + 1} \, dx
\]

Let \(u = e^x\), then \(du = e^x dx\), and \(dx = \frac{du}{u}\). When \(x = 0\), \(u = 1\), and when \(x \to \infty\), \(u \to \infty\). The integral transforms to:
\[
\int_1^\infty \frac{u}{u^2 + 1} \cdot \frac{du}{u} = \int_1^\infty \frac{1}{u^2 + 1} \, du
\]

This is a standard integral:
\[
\int \frac{1}{u^2 + 1} \, du = \arctan(u) + C
\]

Evaluating from 1 to \(\infty\):
\[
\left[ \arctan(u) \right]_1^\infty = \arctan(\infty) - \arctan(1) = \frac{\pi}{2} - \frac{\pi}{4} = \frac{\pi}{4}
\]

#### Second Integral:
\[
\int_0^\infty \frac{e^{-x}}{e^{2x} + 1} \, dx
\]

Let \(v = e^{-x}\), then \(dv = -e^{-x} dx\), and \(dx = -\frac{dv}{v}\). When \(x = 0\), \(v = 1\), and when \(x \to \infty\), \(v \to 0\). The integral transforms to:
\[
\int_1^0 \frac{v}{\frac{1}{v^2} + 1} \cdot \left(-\frac{dv}{v}\right) = \int_0^1 \frac{v^2}{1 + v^2} \, dv
\]

This can be simplified:
\[
\int_0^1 \frac{v^2}{1 + v^2} \, dv = \int_0^1 \left(1 - \frac{1}{1 + v^2}\right) \, dv = \int_0^1 1 \, dv - \int_0^1 \frac{1}{1 + v^2} \, dv
\]

Evaluating these integrals:
\[
\int_0^1 1 \, dv = 1
\]
\[
\int_0^1 \frac{1}{1 + v^2} \, dv = \arctan(v) \Big|_0^1 = \arctan(1) - \arctan(0) = \frac{\pi}{4} - 0 = \frac{\pi}{4}
\]

Thus:
\[
\int_0^1 \frac{v^2}{1 + v^2} \, dv = 1 - \frac{\pi}{4}
\]

### Combining the Results

Combining the results of the two integrals:
\[
\int_0^\infty \frac{\tanh(x)}{e^x} \, dx = \frac{\pi}{4} - \left(1 - \frac{\pi}{4}\right) = \frac{\pi}{4} - 1 + \frac{\pi}{4} = \frac{\pi}{2} - 1
\]

### Step 2: Numerical Approximation

The numerical approximation of \(\frac{\pi}{2} - 1\) is:
\[
\frac{\pi}{2} \approx 1.57079632679
\]
\[
\frac{\pi}{2} - 1 \approx 0.57079632679
\]

### Step 3: JSON Output

\[
\boxed{
\begin{aligned}
\text{"answer": "}\frac{\pi}{2} - 1\text{"}, \\
\text{"numerical_answer": "0.5707963268"}
\end{aligned}
}
\]