We wish to evaluate

  I = ∫₀² x^(1/2) (2 − x)^(−1/2) cos(√(x(2 − x))) dx.

A very useful substitution is x = 2 sin²θ. Notice that when x goes from 0 to 2, we have
  θ = 0  and  θ = π/2.

Step 1. Change of Variable

Let
  x = 2 sin²θ  ⇒  dx = 4 sinθ cosθ dθ.
Then:
  √x = √(2 sin²θ) = √2 sinθ.
Also,
  2 − x = 2 − 2 sin²θ = 2 cos²θ  ⇒  (2 − x)^(−1/2) = 1/√(2 cos²θ) = 1/(√2 cosθ).
Moreover, the product inside the cosine becomes:
  √(x(2 − x)) = √(2 sin²θ · 2 cos²θ) = √(4 sin²θ cos²θ) = 2 sinθ cosθ.
Thus, cos(√(x(2 − x))) becomes cos(2 sinθ cosθ).

Step 2. Substitute into the Integral

Replacing all parts we have:
  I = ∫₀^(π/2) [ (√2 sinθ)/(√2 cosθ) ] · cos(2 sinθ cosθ) · [4 sinθ cosθ dθ ].
The ratio √2 sinθ/(√2 cosθ) simplifies to tanθ. Then:
  I = 4 ∫₀^(π/2) tanθ · sinθ cosθ · cos(2 sinθ cosθ) dθ.
Since tanθ = sinθ/cosθ, the product becomes:
  tanθ · sinθ cosθ = (sinθ/cosθ)· sinθ cosθ = sin²θ.
Hence,
  I = 4 ∫₀^(π/2) sin²θ · cos(2 sinθ cosθ) dθ.

Step 3. A Further Substitution

Write u = 2θ so that du = 2 dθ. When θ = 0, u = 0; when θ = π/2, u = π. Note that
  sin²θ = sin²(u/2)
and that
  2 sinθ cosθ = sin2θ = sin u.
Also, dθ = du/2. Therefore,
  I = 4 ∫₀^π sin²(u/2) · cos(sin u) · (du/2) = 2 ∫₀^π sin²(u/2) cos(sin u) du.
Using the half-angle identity:
  sin²(u/2) = (1 − cos u)/2,
we get:
  I = 2 ∫₀^π [(1 − cos u)/2] cos(sin u) du = ∫₀^π (1 − cos u) cos(sin u) du.
Thus, we split I into two parts:
  I = ∫₀^π cos(sin u) du − ∫₀^π cos u · cos(sin u) du.

Step 4. Recognize Standard Integrals

It is known that (see, e.g., standard integral tables or treat via Fourier–Bessel representations)
  ∫₀^π cos(z sin u) du = π J₀(z).
For z = 1, this gives:
  A = ∫₀^π cos(sin u) du = π J₀(1).

Also, a more general result is:
  ∫₀^π cos(nu) cos(z sin u) du = π Jₙ(z)
for nonnegative integer n. With n = 1 and z = 1 we obtain:
  B = ∫₀^π cos u · cos(sin u) du = π J₁(1).

Thus, the original integral becomes:
  I = π J₀(1) − π J₁(1) = π [J₀(1) − J₁(1)].

This is the exact analytic answer.

Step 5. Numerical Approximation

The usual numerical values for the Bessel functions are approximately:
  J₀(1) ≈ 0.7651976866  and  J₁(1) ≈ 0.4400505857.
Thus,
  J₀(1) − J₁(1) ≈ 0.3251471009.
Then,
  I ≈ π · 0.3251471009 ≈ 3.1415926536 × 0.3251471009 ≈ 1.0210320333.

Step 6. Final Answer in JSON Format

{"answer": "$\\pi\\left(J_0(1)-J_1(1)\\right)$", "numerical_answer": "1.0210320333"}