We will show one way to obtain an answer in closed‐form for

  I = ∫₀¹ arccos(x) · arctan(x) dx.

Step 1. Begin with
  I = ∫₀¹ arccos x · arctan x dx.

A good idea is to use integration by parts. In our solution we take

  u = arctan x   and  dv = arccos x dx.

Then
  du = (1/(1+x²)) dx,
and we need an antiderivative for dv. A standard formula gives
  ∫ arccos x dx = x arccos x − √(1−x²) + C.
Thus, we can take
  v = x arccos x − √(1−x²).

Now the integration‐by‐parts formula gives:

  I = [u v]₀¹ − ∫₀¹ v · du
    = [ arctan x (x arccos x − √(1−x²)) ]₀¹ − ∫₀¹ (x arccos x − √(1−x²))/(1+x²) dx.

A short calculation shows that the boundary terms vanish (at x = 1, note that arccos1 = 0; at x = 0, arctan 0 = 0). Hence

  I = −∫₀¹ (x arccos x − √(1−x²))/(1+x²) dx
    = ∫₀¹ [√(1−x²)/(1+x²)] dx − ∫₀¹ [x arccos x/(1+x²)] dx.

Denote these two integrals by

  I₁ = ∫₀¹ √(1−x²)/(1+x²) dx  and  I₂ = ∫₀¹ x arccos x/(1+x²) dx.

Step 2. We now evaluate I₁.

Make the substitution x = sinθ so that dx = cosθ dθ and √(1−x²) = cosθ. When x goes from 0 to 1, θ goes from 0 to π/2. Then

  I₁ = ∫₀^(π/2) (cosθ·cosθ)/(1+sin²θ) dθ = ∫₀^(π/2) (cos²θ)/(1+sin²θ)dθ.

Write cos²θ = 1 − sin²θ. Thus

  I₁ = ∫₀^(π/2) [1/(1+sin²θ) − sin²θ/(1+sin²θ)] dθ.
But note that
  ∫₀^(π/2) sin²θ/(1+sin²θ)dθ = ∫₀^(π/2)[1 − 1/(1+sin²θ)] dθ.
Thus
  I₁ = 2∫₀^(π/2) [1/(1+sin²θ)] dθ − (π/2).

There is a standard formula:
  ∫₀^(π/2) dθ/(1+m sin²θ) = (π/2)/√(1+m).
For m = 1 we have
  ∫₀^(π/2) dθ/(1+ sin²θ) = (π/2)/√2.
Hence,
  I₁ = 2·((π/2)/√2) − (π/2) = (π/√2) − (π/2)
    = π (1/√2 − 1/2).

Step 3. Next, we evaluate I₂.

Write
  I₂ = ∫₀¹ [x arccos x/(1+x²)] dx.
A good change of variable is u = arccos x so that x = cos u and dx = − sin u du. When x goes from 0 to 1, u goes from arccos 0 = π/2 to arccos 1 = 0. Changing the limits we obtain

  I₂ = ∫_(u=π/2)^(0) [cos u · u/(1+cos²u)] (− sin u du)
    = ∫₀^(π/2) [u cos u sin u/(1+cos²u)] du.
Notice that cos u sin u = (1/2) sin 2u so that

  I₂ = (1/2) ∫₀^(π/2) [u sin 2u/(1+cos²u)] du.

Write cos²u in terms of cos 2u; since
  cos²u = (1+cos2u)/2,
we have
  1+cos²u = 1 + (1+cos2u)/2 = (3+cos2u)/2.
Therefore, the factor 1/(1+cos²u) becomes 2/(3+cos2u) and

  I₂ = (1/2) ∫₀^(π/2) [u sin 2u · (2/(3+cos2u))] du = ∫₀^(π/2) [u sin 2u/(3+cos2u)] du.

Now perform the substitution t = cos2u, so that dt = −2 sin2u du or sin2u du = − dt/2. Also, note that 2u = arccos t so that u = (1/2) arccos t. When u = 0, t = cos0 = 1; when u = π/2, t = cosπ = −1. Then

  I₂ = ∫_(t=1)^(−1) [(1/2) arccos t · (−dt/2)/(3+t)]
    = (1/4) ∫_(t=−1)^(1) [arccos t/(3+t)] dt.
That is,
  I₂ = (1/4) J,  where  J = ∫_(−1)^(1) [arccos t/(3+t)] dt.

To evaluate J, change variable once more by letting u = arccos t so that t = cos u and dt = − sin u du; when t = −1, u = π and when t = 1, u = 0. Then

  J = ∫_(u=π)^(0) [u/(3+cos u)] (− sin u du)
    = ∫₀^(π) [u sin u/(3+cos u)] du.
Now integrate by parts: let
  w = u  ⇒ dw = du,  and dv = sin u/(3+cos u) du.
Observe that
  d/du ln(3+cos u) = − sin u/(3+cos u).
Thus, an antiderivative for dv is
  v = − ln(3+cos u).
Then by integration by parts

  J = [u·(− ln(3+cos u))]₀^(π) − ∫₀^(π)[− ln(3+cos u)] du
    = −π ln(3+cos π) + ∫₀^(π) ln(3+cos u) du.
Since cos π = −1, we have 3+cos π = 2 so that the boundary term is −π ln 2. Also, a standard formula tells us that
  ∫₀^(π) ln(a+ b cos u) du = π ln[(a+√(a²−b²))/2],  for a > |b|.
Here a = 3 and b = 1 so that
  ∫₀^(π) ln(3+cos u) du = π ln((3+√8)/2) = π ln((3+2√2)/2).
Thus,
  J = π [ln((3+2√2)/2) − ln 2] = π ln((3+2√2)/4).
Then,
  I₂ = (1/4) J = (π/4) ln((3+2√2)/4).

Step 4. We now combine the pieces. We had

  I = I₁ − I₂ = π (1/√2 − 1/2) − (π/4) ln((3+2√2)/4).

This is an acceptable exact answer. (Note that one may also write 1/√2 − 1/2 = (2 − √2)/(2√2).)

Step 5. A numerical approximation.

Let us compute:
  √2 ≈ 1.4142135624.
Then:
  1/√2 − 1/2 ≈ (0.7071067812 − 0.5) = 0.2071067812.
Multiply by π:
  π(1/√2 − 1/2) ≈ 3.1415926536 × 0.2071067812 ≈ 0.6506450169.
Next, compute (3+2√2):
  3 + 2×1.4142135624 ≈ 5.8284271248.
Then (3+2√2)/4 ≈ 5.8284271248/4 ≈ 1.4571067812.
Taking the logarithm:
  ln(1.4571067812) ≈ 0.376201.
Multiplying by π/4:
  (π/4) ln((3+2√2)/4) ≈ 0.7853981634 × 0.376201 ≈ 0.295405.
Thus, the final numerical value is
  I ≈ 0.6506450169 − 0.295405 ≈ 0.3552400169.

Step 6. Final Answer

In summary, one acceptable answer is

  I = (π(2−√2))/(2√2) − (π/4) ln((3+2√2)/4).

Numerically, I ≈ 0.3552400169.

The final answer in the required JSON format is shown on the last line below.

{"answer": "\\frac{\\pi (2-\\sqrt{2})}{2\\sqrt{2}}-\\frac{\\pi}{4}\\ln\\frac{3+2\\sqrt{2}}{4}", "numerical_answer": "0.3552400169"}