Let’s compute the integral:
\[
I = \int_{0}^{1} x^3 \arccos x \, [\arcsin x]^2 \, dx
\]

**Step 1: Substitution to Simplify**

Let \( x = \sin\theta \), where \( \theta \) goes from \( 0 \) to \( \frac{\pi}{2} \) as \( x \) goes from \( 0 \) to \( 1 \).

Then:
- \( dx = \cos\theta\, d\theta \)
- \( x^3 = \sin^3\theta \)
- \( \arccos x = \arccos(\sin\theta) = \frac{\pi}{2} - \theta \)
- \( \arcsin x = \arcsin(\sin\theta) = \theta \)
- Thus, \( [\arcsin x]^2 = \theta^2 \)

The integral becomes:

\[
I = \int_{x=0}^{x=1} x^3 \arccos x \arcsin^2 x \, dx
  = \int_{\theta=0}^{\theta=\frac{\pi}{2}} \sin^3\theta \cdot \left(\frac{\pi}{2} - \theta\right) \cdot \theta^2 \cdot \cos\theta\, d\theta
\]

\[
I = \int_{0}^{\frac{\pi}{2}} \sin^3\theta \cos\theta \, \left(\frac{\pi}{2} - \theta \right) \theta^2 d\theta
\]

Let’s expand:
\[
I = \frac{\pi}{2} \int_{0}^{\frac{\pi}{2}} \sin^3\theta \cos\theta \, \theta^2 d\theta - \int_{0}^{\frac{\pi}{2}} \sin^3\theta \cos\theta \, \theta^3 d\theta
\]

So,
\[
I = \frac{\pi}{2} I_1 - I_2
\]
where
\[
I_1 = \int_{0}^{\frac{\pi}{2}} \sin^3\theta \cos\theta \, \theta^2 d\theta
\]
and
\[
I_2 = \int_{0}^{\frac{\pi}{2}} \sin^3\theta \cos\theta \, \theta^3 d\theta
\]

**Step 2: Compute \( I_1 \) and \( I_2 \) by Integration by Parts**

Let’s consider \( I_n = \int_{0}^{\frac{\pi}{2}} \sin^3\theta \cos\theta \, \theta^n \, d\theta \).

Let’s use integration by parts for a generic \( n \):

Let 
- \( u = \theta^n \), \( du = n \theta^{n-1} d\theta \)
- \( dv = \sin^3\theta \cos\theta \, d\theta \), \( v = \int \sin^3\theta \cos\theta \, d\theta \)

Let’s compute \( v = \int \sin^3\theta \cos\theta\, d\theta \):

Set \( t = \sin\theta \), \( dt = \cos\theta d\theta \), so,
\[
\int \sin^3\theta \cos\theta d\theta = \int t^3 dt = \frac{t^4}{4} = \frac{\sin^4\theta}{4}
\]

So, by integration by parts,
\[
I_n = \left[ \frac{\sin^4\theta}{4} \cdot \theta^n \right]_{0}^{\frac{\pi}{2}} - \int_{0}^{\frac{\pi}{2}} \frac{\sin^4\theta}{4} \cdot n \theta^{n-1} d\theta
\]
\[
= \left[ \frac{\sin^4\theta}{4} \cdot \theta^n \right]_{0}^{\frac{\pi}{2}} - \frac{n}{4} \int_{0}^{\frac{\pi}{2}} \sin^4\theta \, \theta^{n-1} d\theta
\]
But at the endpoints:
- At \( \theta = 0 \): \( \sin^4 0 = 0 \)
- At \( \theta = \frac{\pi}{2} \): \( \sin^4 (\frac{\pi}{2}) = 1 \)

So,
\[
\left[ \frac{\sin^4\theta}{4} \cdot \theta^n \right]_{0}^{\frac{\pi}{2}} = \frac{1}{4}\left( \frac{\pi}{2} \right)^n - 0
\]
Therefore,
\[
I_n = \frac{1}{4} \left( \frac{\pi}{2} \right)^n - \frac{n}{4} J_{n-1}
\]
where
\[
J_{n-1} = \int_{0}^{\frac{\pi}{2}} \sin^4\theta \, \theta^{n-1} d\theta
\]

Let's apply it to \( n=2 \) and \( n=3 \):

First, \( I_1 \):

But let's keep it for \( n=2,3 \):

**For \( n=2 \):**
\[
I_2 = \frac{1}{4}\left(\frac{\pi}{2}\right)^2 - \frac{2}{4} J_1 = \frac{\pi^2}{16} - \frac{1}{2} J_1
\]
where \( J_1 = \int_{0}^{\frac{\pi}{2}} \sin^4\theta \, \theta d\theta \)

Similarly, for \( n=3 \):

\[
I_3 = \frac{1}{4}\left(\frac{\pi}{2}\right)^3 - \frac{3}{4} J_2 = \frac{\pi^3}{32} - \frac{3}{4} J_2
\]
where \( J_2 = \int_{0}^{\frac{\pi}{2}} \sin^4\theta \, \theta^2 d\theta \)

Recall:
\[
I = \frac{\pi}{2} I_1 - I_2
\]
But we have \( I_1 \) and \( I_2 \) in terms of \( J_0, J_1 \):

Let’s first write \( I_1 \):

\[
I_1 = \int_{0}^{\frac{\pi}{2}} \sin^3\theta \cos\theta \, \theta^2 d\theta
= \frac{1}{4} \left( \frac{\pi}{2} \right)^2 - \frac{2}{4} \int_{0}^{\frac{\pi}{2}} \sin^4\theta \theta d\theta
= \frac{\pi^2}{16} - \frac{1}{2} J_1
\]

Similarly,
\[
I_2 = \int_{0}^{\frac{\pi}{2}} \sin^3\theta \cos\theta \, \theta^3 d\theta
= \frac{\pi^3}{32} - \frac{3}{4} J_2
\]

So,

\[
I = \frac{\pi}{2} I_1 - I_2 = \frac{\pi}{2} \left( \frac{\pi^2}{16} - \frac{1}{2} J_1 \right) - \left( \frac{\pi^3}{32} - \frac{3}{4} J_2 \right )
\]
\[
= \frac{\pi^3}{32} - \frac{\pi}{4} J_1 - \frac{\pi^3}{32} + \frac{3}{4} J_2
\]
\[
= -\frac{\pi}{4} J_1 + \frac{3}{4} J_2
\]

Therefore,

\[
\boxed{I = \frac{3}{4} J_2 - \frac{\pi}{4} J_1}
\]

where

\[
J_n = \int_{0}^{\frac{\pi}{2}} \sin^4\theta \, \theta^n d\theta
\]

**Step 3: Express \( \sin^4\theta \) in Terms of Cosines**

Recall:
\[
\sin^4\theta = \left( \sin^2\theta \right)^2 = \left( \frac{1 - \cos 2\theta}{2} \right)^2 = \frac{1}{4}(1 - 2\cos2\theta + \cos^2 2\theta)
\]
But
\[
\cos^2 2\theta = \frac{1 + \cos 4\theta}{2}
\]
Thus,
\[
\sin^4\theta = \frac{1}{4} \left(1 - 2\cos2\theta + \frac{1 + \cos4\theta}{2}\right)
= \frac{1}{4}\left(1 - 2\cos2\theta + \frac{1}{2} + \frac{1}{2}\cos4\theta\right)
= \frac{3}{8} - \frac{1}{2} \cos 2\theta + \frac{1}{8} \cos 4\theta
\]

Therefore,

\[
J_n = \int_{0}^{\frac{\pi}{2}} \left( \frac{3}{8} - \frac{1}{2}\cos 2\theta + \frac{1}{8}\cos 4\theta \right) \theta^n d\theta
\]
\[
= \frac{3}{8} \int_{0}^{\frac{\pi}{2}} \theta^n d\theta - \frac{1}{2} \int_{0}^{\frac{\pi}{2}} \cos 2\theta \theta^n d\theta + \frac{1}{8} \int_{0}^{\frac{\pi}{2}} \cos 4\theta \theta^n d\theta
\]

Let’s compute \( J_1 \) and \( J_2 \):

**First, \( J_1 \):**

\[
J_1 = \frac{3}{8} \int_0^{\frac{\pi}{2}} \theta d\theta - \frac{1}{2} \int_0^{\frac{\pi}{2}} \cos 2\theta \, \theta d\theta + \frac{1}{8} \int_0^{\frac{\pi}{2}} \cos 4\theta \, \theta d\theta
\]

- \( \int_{0}^{a} \theta d\theta = \frac{1}{2} a^2 \)
- \( \int_0^a \cos (k\theta) \theta d\theta \) can be found by integration by parts.

First,
\[
A_1 = \int_0^{\frac{\pi}{2}} \theta d\theta = \left.\frac{1}{2}\theta^2\right|_0^{\frac{\pi}{2}} = \frac{1}{2} \left(\frac{\pi}{2}\right)^2 = \frac{\pi^2}{8}
\]

\[
A_2 = \int_0^{\frac{\pi}{2}} \cos 2\theta \, \theta d\theta
\]
Do by parts:
Let \( u = \theta, dv = \cos 2\theta d\theta \);
then \( du = d\theta, v = \frac{1}{2} \sin 2\theta \).

Thus
\[
A_2 = \left. \frac{1}{2} \theta \sin 2\theta \right|_0^{\frac{\pi}{2}} - \int_0^{\frac{\pi}{2}} \frac{1}{2} \sin 2\theta d\theta
\]
\[
= 0 - \frac{1}{2} \int_{0}^{\frac{\pi}{2}} \sin 2\theta d\theta
\]
But \( \int \sin 2\theta d\theta = -\frac{1}{2} \cos 2\theta \), so

\[
A_2 = -\frac{1}{2}\left( -\frac{1}{2}[\cos 2\theta]_0^{\frac{\pi}{2}} \right)
= \frac{1}{4}\left( \cos 2\theta \Big|_0^{\frac{\pi}{2}} \right)
= \frac{1}{4}( \cos \pi - \cos 0 ) = \frac{1}{4}( -1 - 1 ) = -\frac{1}{2}
\]

Next,
\[
A_3 = \int_0^{\frac{\pi}{2}} \cos 4\theta \, \theta d\theta
\]
Again by parts:

Let \( u = \theta, dv = \cos 4\theta d\theta \)
Then \( du = d\theta, v = \frac{1}{4} \sin 4\theta \)

\[
A_3 = \left. \frac{1}{4} \theta \sin 4\theta \right|_0^{\frac{\pi}{2}} - \int_0^{\frac{\pi}{2}} \frac{1}{4} \sin 4\theta d\theta
\]
\[
= 0 - \frac{1}{4} \int_0^{\frac{\pi}{2}} \sin 4\theta d\theta
\]
But \( \int \sin 4\theta d\theta = -\frac{1}{4} \cos 4\theta \)
So,

\[
A_3 = -\frac{1}{4} \left( -\frac{1}{4} [\cos 4\theta]_0^{\frac{\pi}{2}} \right )
= \frac{1}{16} ( \cos 4\theta |_0^{\frac{\pi}{2}} )
= \frac{1}{16} ( \cos 2\pi - \cos 0 ) = \frac{1}{16} ( 1 - 1 ) = 0
\]

Therefore,
\[
J_1 = \frac{3}{8} \cdot \frac{\pi^2}{8} - \frac{1}{2} \cdot ( -\frac{1}{2} ) + 0
= \frac{3\pi^2}{64} + \frac{1}{4}
\]

**Now, \( J_2 \):**

\[
J_2 = \frac{3}{8} \int_0^{\frac{\pi}{2}} \theta^2 d\theta - \frac{1}{2} \int_0^{\frac{\pi}{2}} \cos 2\theta\, \theta^2 d\theta + \frac{1}{8} \int_0^{\frac{\pi}{2}} \cos 4\theta\, \theta^2 d\theta
\]

First,
\[
B_1 = \int_0^{\frac{\pi}{2}} \theta^2 d\theta = \left. \frac{1}{3} \theta^3 \right|_0^{\frac{\pi}{2}} = \frac{1}{3} \left(\frac{\pi}{2}\right)^3 = \frac{\pi^3}{24}
\]

Second,
\[
B_2 = \int_0^{\frac{\pi}{2}} \cos 2\theta \, \theta^2 d\theta
\]

Integrate by parts:
Let \( u = \theta^2, dv = \cos 2\theta d\theta \)
Then \( du = 2\theta d\theta, v = \frac{1}{2} \sin 2\theta \)

\[
B_2 = \left. \frac{1}{2} \theta^2 \sin 2\theta \right|_0^{\frac{\pi}{2}} - \int_0^{\frac{\pi}{2}} \frac{1}{2} \sin 2\theta \cdot 2\theta d\theta
= 0 - \int_0^{\frac{\pi}{2}} \sin 2\theta \, \theta d\theta
\]

Let’s evaluate \( S = \int_0^{\frac{\pi}{2}} \theta \sin 2\theta d\theta \)

Integration by parts:

Let \( u = \theta, dv = \sin 2\theta d\theta \)
Then \( du = d\theta, v = -\frac{1}{2}\cos 2\theta \)

\[
S = \left. -\frac{1}{2} \theta \cos 2\theta \right|_0^{\frac{\pi}{2}} + \int_0^{\frac{\pi}{2}} \frac{1}{2} \cos 2\theta d\theta
= -\frac{1}{2} \left( \frac{\pi}{2} \cos \pi - 0 \right ) + \frac{1}{2} \cdot \int_0^{\frac{\pi}{2}} \cos 2\theta d\theta
\]

But \( \int_0^{\frac{\pi}{2}} \cos 2\theta d\theta = \left.\frac{1}{2} \sin 2\theta \right|_0^{\frac{\pi}{2}} = 0 \)

Also, \( \cos \pi = -1 \), so

\[
S = -\frac{1}{2} \cdot \frac{\pi}{2} (-1) + 0 = \frac{\pi}{4}
\]

Therefore,
\[
B_2 = -S = -\frac{\pi}{4}
\]

Third,

\[
B_3 = \int_0^{\frac{\pi}{2}} \cos 4\theta \, \theta^2 d\theta
\]

Again, integrate by parts:

First, \( u = \theta^2 \), \( dv = \cos 4\theta d\theta \)
\( du = 2\theta d\theta \), \( v = \frac{1}{4} \sin 4\theta \)

\[
B_3 = \left. \frac{1}{4} \theta^2 \sin 4\theta \right|_0^{\frac{\pi}{2}} - \int_0^{\frac{\pi}{2}} \frac{1}{4} \sin 4\theta \cdot 2\theta d\theta
= 0 - \frac{1}{2} \int_0^{\frac{\pi}{2}} \sin 4\theta \, \theta d\theta
\]

Let’s compute \( T = \int_0^{\frac{\pi}{2}} \theta \sin 4\theta d\theta \)

By parts, \( u = \theta, dv = \sin 4\theta d\theta \)
\( du = d\theta, v = -\frac{1}{4} \cos 4\theta \)
\[
T = -\frac{1}{4} \theta \cos 4\theta \Big|_0^{\frac{\pi}{2}} + \int_0^{\frac{\pi}{2}} \frac{1}{4} \cos 4\theta d\theta
= -\frac{1}{4} \cdot \frac{\pi}{2} \cos 2\pi + 0 + \frac{1}{4} \cdot \int_0^{\frac{\pi}{2}} \cos 4\theta d\theta
\]
But \( \int_0^{\frac{\pi}{2}} \cos 4\theta d\theta = \left. \frac{1}{4} \sin 4\theta \right|_0^{\frac{\pi}{2}} = 0 \)

Also, \( \cos 2\pi = 1 \)

So,
\[
T = -\frac{1}{4} \cdot \frac{\pi}{2} \cdot 1 = -\frac{\pi}{8}
\]
Thus,
\[
B_3 = -\frac{1}{2} T = -\frac{1}{2} \cdot ( -\frac{\pi}{8} ) = \frac{\pi}{16}
\]

Now, collect the terms:
\[
J_2 = \frac{3}{8} \cdot \frac{\pi^3}{24} - \frac{1}{2} \cdot ( -\frac{\pi}{4}) + \frac{1}{8} \cdot \frac{\pi}{16}
= \frac{3\pi^3}{192} + \frac{\pi}{8} + \frac{\pi}{128}
= \frac{\pi^3}{64} + \frac{\pi}{8} + \frac{\pi}{128}
\]
But,
\[
\frac{\pi}{8} + \frac{\pi}{128} = \frac{16\pi + \pi}{128} = \frac{17\pi}{128}
\]
So,
\[
J_2 = \frac{\pi^3}{64} + \frac{17\pi}{128}
\]

Now, plug in \( J_1 \) and \( J_2 \) into the formula for \( I \):

Recall:
\[
I = \frac{3}{4} J_2 - \frac{\pi}{4} J_1
\]

Insert \( J_2 \) and \( J_1 \) from above:
\[
J_2 = \frac{\pi^3}{64} + \frac{17\pi}{128}
\]
\[
J_1 = \frac{3\pi^2}{64} + \frac{1}{4}
\]

First,
\[
\frac{3}{4} J_2 = \frac{3}{4} \left( \frac{\pi^3}{64} + \frac{17\pi}{128} \right ) = \frac{3\pi^3}{256} + \frac{51 \pi}{512}
\]
Second,
\[
\frac{\pi}{4} J_1 = \frac{\pi}{4} \left( \frac{3\pi^2}{64} + \frac{1}{4} \right ) = \frac{3\pi^3}{256} + \frac{\pi}{16}
\]
Therefore,

\[
I = \left( \frac{3\pi^3}{256} + \frac{51\pi}{512} \right ) - \left( \frac{3 \pi^3}{256} + \frac{\pi}{16} \right ) = \frac{51\pi}{512} - \frac{\pi}{16} = \frac{51\pi - 32\pi}{512} = \frac{19\pi}{512}
\]

**Final Exact Answer:**
\[
\boxed{I = \frac{19\pi}{512}}
\]

**Step 4: Numerical Approximation**

Now, \( \pi \approx 3.14159265359 \), so

\[
I \approx \frac{19 \cdot 3.14159265359}{512} \approx \frac{59.6902604182}{512} \approx 0.1166298039
\]

**Step 5: JSON Output**

```json
{"answer": "\\frac{19\\pi}{512}", "numerical_answer": "0.1166298039"}
```