<think>
Okay, so I need to compute the definite integral of sin(101x) times sin(x) raised to the 99th power. Hmm, that's ∫ sin(101x) sin^99(x) dx. Let me think about how to approach this. 

First, integrating products of trigonometric functions often involves using identities to simplify the expression. The product of sines here might be tricky because of the high exponent. Maybe I can use some trigonometric identities to rewrite sin^99(x) in a more manageable form. Wait, there's the power-reduction formula, but that might get complicated with such a high power. Alternatively, perhaps using complex exponentials? Euler's formula comes to mind, where sin(x) = (e^(ix) - e^(-ix))/(2i). Maybe expanding sin^99(x) using the binomial theorem? That seems like a lot of terms, but maybe there's a pattern or cancellation when multiplied by sin(101x).

Alternatively, maybe there's a recursive formula for integrating sin^n(x) terms. But with the sin(101x) multiplied in, I need to see if there's a way to combine these terms. Let me recall the product-to-sum identities. The identity for sin A sin B is [cos(A-B) - cos(A+B)] / 2. But here, we have sin(101x) multiplied by sin^99(x). So maybe I can apply the product-to-sum identity multiple times?

Wait, but sin^99(x) is a product of 99 sine terms. That's a lot. Maybe there's a pattern when you multiply multiple sines. Alternatively, perhaps using the identity for sin(nx) in terms of powers of sin(x). But I'm not sure. Let me think.

Another approach: consider integrating over a symmetric interval. Wait, but the problem says definite integral, but the user didn't specify the limits. Wait, wait, the original problem is to compute the definite integral ∫ sin(101x) sin^99(x) dx. Wait, hold on, the user wrote "definite integral" but didn't specify the limits. That's confusing. Wait, maybe it's an indefinite integral? But the problem says "definite integral". Hmm, perhaps there's a typo or maybe the limits are from 0 to 2π or something? Wait, maybe the user intended an indefinite integral but wrote definite. Wait, the problem says "definite integral" but the integral is written without limits. That's inconsistent. Maybe the user made a mistake. Wait, but the problem says "Please calculate the definite integral ∫ sin(101x) sin^{99}(x) dx." So maybe it's actually an integral over the entire real line or a specific interval? Wait, without limits, it's unclear. But the user might have intended an indefinite integral. Wait, but the problem statement says "definite integral", which requires limits. Hmm. Maybe there's a standard interval for such problems, like 0 to 2π? Because integrating over a full period might lead to simplifications. Let me check.

If the integral is over 0 to 2π, then perhaps we can use orthogonality of sine functions. For example, ∫₀^{2π} sin(nx) sin(mx) dx = 0 if n ≠ m and π if n = m. But here, we have sin(101x) multiplied by sin^99(x). So sin^99(x) can be expressed as a sum of sines of multiple angles. Then, when multiplied by sin(101x), integrating over 0 to 2π would pick out the term where the frequency matches 101. That might be the key.

So, first, express sin^99(x) as a Fourier series, i.e., a sum of sines and cosines of multiple angles. Then, multiply by sin(101x) and integrate term by term. The only term that would survive is the one where the frequency matches 101. So the integral would be non-zero only if there's a term in the expansion of sin^99(x) that has sin(101x) or cos(101x), but since we're multiplying by sin(101x), the product would have terms like sin(101x) sin(kx) or sin(101x) cos(kx). The integral over 0 to 2π of sin(101x) cos(kx) is zero, and the integral of sin(101x) sin(kx) is zero unless k=101, in which case it's π. So the integral would be π times the coefficient of sin(101x) in the expansion of sin^99(x). Wait, but sin^99(x) is an odd function, so its Fourier series would consist of sine terms only. Therefore, the integral would be the coefficient of sin(101x) in sin^99(x) multiplied by π.

So the problem reduces to finding the coefficient of sin(101x) in the expansion of sin^99(x). How do we find that?

To expand sin^99(x) as a sum of sines, we can use the identity for sin^n(x). For odd exponents, sin^{2m+1}(x) can be written as a sum of sin((2k+1)x) terms. The general formula for sin^n(x) when n is odd is a combination of sines of odd multiples of x. Let me recall the formula.

The expansion of sin^n(x) for odd n=2m+1 is given by:

sin^{2m+1}(x) = (1/2^{2m}) Σ_{k=0}^{m} (-1)^k C(2m+1, m - k) sin((2k+1)x)

Wait, I need to check the exact coefficients. Alternatively, using complex exponentials might be more straightforward. Let's express sin(x) as (e^{ix} - e^{-ix})/(2i), then raise it to the 99th power.

So sin^99(x) = [ (e^{ix} - e^{-ix}) / (2i) ) ]^99.

Expanding this using the binomial theorem:

= (1/(2i)^99) Σ_{k=0}^{99} C(99, k) (-1)^{99 - k} e^{i(99 - 2k)x}

Because each term in the expansion is (e^{ix})^k ( -e^{-ix} )^{99 -k} = (-1)^{99 -k} e^{i( k - (99 -k) )x} = (-1)^{99 -k} e^{i(2k -99)x}

Wait, let me check that. The expansion of (a + b)^n is Σ_{k=0}^n C(n, k) a^{k} b^{n -k}. Here, a = e^{ix}, b = -e^{-ix}, n=99. So each term is C(99, k) (e^{ix})^k (-e^{-ix})^{99 -k} = C(99, k) (-1)^{99 -k} e^{i x k} e^{-i x (99 -k)} = C(99, k) (-1)^{99 -k} e^{i x (k - (99 -k))} = C(99, k) (-1)^{99 -k} e^{i x (2k -99)}.

Therefore, sin^99(x) = (1/(2i)^99}) Σ_{k=0}^{99} C(99, k) (-1)^{99 -k} e^{i(2k -99)x}

But we can write e^{i(2k -99)x} = e^{i m x} where m = 2k -99. So the exponents are m = 2k -99. Since k ranges from 0 to 99, m ranges from 2*0 -99 = -99 to 2*99 -99 = 99. So m ranges from -99 to 99 in steps of 2. Therefore, the expansion is a sum of exponentials e^{i m x} with m odd (since 2k -99 is odd when 99 is odd). Therefore, sin^99(x) can be written as a sum of sin(mx) terms, since the exponentials combine into sine terms due to the imaginary coefficients.

But let's express this sum in terms of sines. Since e^{i m x} - e^{-i m x} = 2i sin(mx), but in our case, the sum includes both positive and negative m. Let's see:

The sum Σ_{k=0}^{99} C(99, k) (-1)^{99 -k} e^{i(2k -99)x} can be rewritten by changing the index. Let m = k - 99/2, but since 99 is odd, maybe it's better to pair terms. Alternatively, note that for each term with exponent m, there is a term with exponent -m when k' = 99 -k. Let's check:

If k' = 99 -k, then m' = 2k' -99 = 2(99 -k) -99 = 198 -2k -99 = 99 -2k. But original m for k is 2k -99. So m' = - (2k -99) = -m. Therefore, the terms for k and 99 -k are complex conjugates. Therefore, when we combine the terms, the imaginary parts will add up, leading to sine terms.

But perhaps it's easier to convert the entire exponential sum into sine terms. Let's proceed.

The expression is:

sin^99(x) = (1/(2i)^99) Σ_{k=0}^{99} C(99, k) (-1)^{99 -k} e^{i(2k -99)x}

But note that (2i)^99 = 2^99 i^99 = 2^99 (i^{4*24 + 3}) = 2^99 (-i). So 1/(2i)^99 = 1/(2^99 (-i)) = -i / 2^99.

Therefore:

sin^99(x) = (-i / 2^99) Σ_{k=0}^{99} C(99, k) (-1)^{99 -k} e^{i(2k -99)x}

Now, let's write this sum as a sum over m = 2k -99. Let m = 2k -99. Then k = (m +99)/2. Since k must be an integer between 0 and 99, m must be odd integers from -99 to 99. So m ranges from -99 to 99 in steps of 2. Therefore, the sum can be rewritten as:

Σ_{m=-99}^{99} step 2 C(99, (m +99)/2) (-1)^{99 - (m +99)/2} e^{i m x}

But this is only valid when (m +99)/2 is integer, i.e., m is odd. So m = -99, -97, ..., 97, 99.

Therefore, sin^99(x) = (-i / 2^99) Σ_{m odd from -99 to 99} C(99, (m +99)/2) (-1)^{99 - (m +99)/2} e^{i m x}

But we can split the sum into positive and negative m:

= (-i / 2^99) [ Σ_{m=1,3,...,99} C(99, (m +99)/2) (-1)^{99 - (m +99)/2} e^{i m x} + Σ_{m=-1,-3,...,-99} C(99, (m +99)/2) (-1)^{99 - (m +99)/2} e^{i m x} ]

For the negative m terms, let m = -n where n is positive odd integer from 1 to 99. Then:

Σ_{m=-1,-3,...,-99} C(99, (-n +99)/2) (-1)^{99 - (-n +99)/2} e^{-i n x}

But (-n +99)/2 = (99 -n)/2. Since n is odd, 99 -n is even, so (99 -n)/2 is integer. Also, note that C(99, (99 -n)/2) = C(99, (99 -n)/2). But since C(n, k) = C(n, n -k), so C(99, (99 -n)/2) = C(99, 99 - (99 -n)/2) = C(99, (99 +n)/2). Wait, but (99 +n)/2 may not be integer. Wait, n is odd, so 99 +n is even, so (99 +n)/2 is integer. Wait, but (99 -n)/2 + (99 +n)/2 = 99. So C(99, (99 -n)/2) = C(99, (99 +n)/2). Therefore, the coefficients for m = n and m = -n are related.

But let's compute the term for m = n and m = -n:

For m = n (positive):

Term: C(99, (n +99)/2) (-1)^{99 - (n +99)/2} e^{i n x}

For m = -n:

Term: C(99, (99 -n)/2) (-1)^{99 - (99 -n)/2} e^{-i n x} = C(99, (99 +n)/2) (-1)^{99 - (99 -n)/2} e^{-i n x}

But 99 - (99 -n)/2 = (198 -99 +n)/2 = (99 +n)/2. So the exponent of (-1) is (99 +n)/2.

Therefore, the two terms are:

C(99, (n +99)/2) (-1)^{ (99 - (n +99)/2) } e^{i n x} + C(99, (n +99)/2) (-1)^{ (99 +n)/2 } e^{-i n x}

Wait, since C(99, (99 -n)/2) = C(99, (99 +n)/2) because of the symmetry of binomial coefficients. So both terms have the same binomial coefficient. Let's factor that out:

C(99, (n +99)/2) [ (-1)^{ (99 - (n +99)/2) } e^{i n x} + (-1)^{ (99 +n)/2 } e^{-i n x} ]

Simplify the exponents of (-1):

(99 - (n +99)/2) = (198 -n -99)/2 = (99 -n)/2

Similarly, (99 +n)/2.

So:

[ (-1)^{ (99 -n)/2 } e^{i n x} + (-1)^{ (99 +n)/2 } e^{-i n x} ]

Factor out (-1)^{ (99 -n)/2 }:

(-1)^{ (99 -n)/2 } [ e^{i n x} + (-1)^{ (99 +n)/2 - (99 -n)/2 } e^{-i n x} ]

Compute the exponent in the second term:

(99 +n)/2 - (99 -n)/2 = (99 +n -99 +n)/2 = (2n)/2 = n

So:

(-1)^{ (99 -n)/2 } [ e^{i n x} + (-1)^n e^{-i n x} ]

But (-1)^n e^{-i n x} = e^{-i n x} multiplied by (-1)^n. Let's see:

If n is even, (-1)^n = 1, so we have e^{i n x} + e^{-i n x} = 2 cos(nx)

If n is odd, (-1)^n = -1, so we have e^{i n x} - e^{-i n x} = 2i sin(nx)

But n here is an odd integer (since m ranges over odd numbers), so n is odd. Therefore, (-1)^n = -1, so:

= (-1)^{ (99 -n)/2 } [ e^{i n x} - e^{-i n x} ] = (-1)^{ (99 -n)/2 } * 2i sin(nx)

Therefore, combining back into the expression for sin^99(x):

= (-i / 2^99) Σ_{n=1,3,...,99} C(99, (n +99)/2) * [ (-1)^{ (99 -n)/2 } * 2i sin(nx) ]

Simplify this:

The (-i) and 2i multiply to (-i)(2i) = 2. The 1/2^99 remains.

So:

= (2 / 2^99) Σ_{n=1,3,...,99} C(99, (n +99)/2) (-1)^{ (99 -n)/2 } sin(nx)

Simplify 2 / 2^99 = 1 / 2^{98}

Therefore:

sin^99(x) = (1 / 2^{98}) Σ_{n=1,3,...,99} C(99, (n +99)/2) (-1)^{ (99 -n)/2 } sin(nx)

Now, the original integral is ∫ sin(101x) sin^99(x) dx. If we are integrating over a full period, say from 0 to 2π, then the integral becomes:

∫₀^{2π} sin(101x) sin^99(x) dx = (1 / 2^{98}) Σ_{n=1,3,...,99} C(99, (n +99)/2) (-1)^{ (99 -n)/2 } ∫₀^{2π} sin(101x) sin(nx) dx

But the integral ∫₀^{2π} sin(101x) sin(nx) dx is zero unless n = 101, in which case it's π. However, in our sum, n ranges from 1 to 99 (odd numbers), so 101 is not included. Therefore, all terms in the sum are zero. Therefore, the integral is zero.

Wait, but that can't be right. Wait, but the sum is over n=1,3,...,99. So 101 is not in the sum. Therefore, the integral over 0 to 2π of sin(101x) sin^99(x) dx is zero.

But the problem says "definite integral" without specifying limits. If the integral is over 0 to 2π, then the answer is zero. But if it's an indefinite integral, then the answer would involve a constant of integration. But the problem says "definite integral", so maybe the user intended the integral over 0 to 2π. Alternatively, maybe the integral from -∞ to ∞, but that's not typical for periodic functions. Alternatively, maybe the user made a mistake and meant indefinite integral. But given the problem says "definite", but no limits, perhaps there's a misunderstanding.

Wait, let me check the problem again. The user wrote: "Please calculate the definite integral ∫sin(101x)sin^{99}(x)dx." So they didn't specify the limits, which is necessary for a definite integral. This is a problem. Maybe it's a typo, and they meant indefinite. But the problem says "definite". Alternatively, maybe the integral is over the entire real line, but that's not standard. Alternatively, perhaps the user intended the integral from 0 to 2π, which is a common interval for trigonometric integrals. Given that, and given that the integral over 0 to 2π is zero, as we saw, then the answer would be zero. But let's confirm.

Alternatively, maybe the integral is from -π to π, which is also a common interval. The result would be the same, since the integral over any interval of length 2π would give the same result due to periodicity.

Therefore, assuming the integral is over 0 to 2π, the answer is zero. But let's check if there's another approach.

Alternatively, if the integral is indefinite, then we need to find an antiderivative. But integrating sin(101x) sin^99(x) dx. That seems complicated, but perhaps using substitution or integration by parts. However, given the high exponent, it's more practical to use the Fourier series approach, but for an indefinite integral, the result would be a sum of cosines plus a constant. However, given the complexity, it's more likely that the problem expects the definite integral over 0 to 2π, which is zero.

But the user didn't specify the limits. This is a problem. However, given the problem mentions "definite integral", and given the structure of the integral, it's likely that the intended answer is zero, assuming integration over a full period. Therefore, the exact answer is 0, and the numerical approximation is also 0.0000000000.

But let me verify this again. If we expand sin^99(x) as a sum of sin(nx) terms with n up to 99, then multiplying by sin(101x) and integrating over 0 to 2π, the orthogonality implies that the integral is zero. Therefore, the answer is zero.

Therefore, the exact answer is 0, and the numerical approximation is 0.0000000000.
</think>

{"answer": "0", "numerical_answer": "0.0000000000"}