<think>
Okay, let's tackle this integral step by step. The integral given is from 0 to 2.0 of x^(1/2) times (2.0 - x)^(-1/2) multiplied by a natural logarithm term. The logarithm part looks complicated: ln(1.0√[x(2.0 - x)] + √[1 + 1.0²x(2.0 - x)]). Hmm, first, I need to simplify the integrand if possible.

Let me write the integral more neatly. Let's denote the integrand as:

x^{1/2} (2 - x)^{-1/2} ln(√[x(2 - x)] + √[1 + x(2 - x)}) dx from 0 to 2.

Wait, the 1.0 coefficients can be considered as 1, so maybe that's just for clarity. Let me check the argument of the logarithm. Let's compute the logarithm's argument:

Inside the ln, we have √[x(2 - x)] + √[1 + x(2 - x)]. Let me denote t = x(2 - x). Then the argument becomes √t + √(1 + t). Hmm, that expression √t + √(1 + t) might be related to hyperbolic functions or something else. Wait, if I let √t = sinh(u), then √(1 + t) would be cosh(u), since sinh²u + 1 = cosh²u. Then √t + √(1 + t) = sinh(u) + cosh(u) = e^u. Therefore, ln(e^u) = u. So the logarithm term simplifies to u, which is sinh^{-1}(√t). But sinh^{-1}(z) = ln(z + √(z² + 1)), which is exactly the form here. Wait, but here we have √t + √(1 + t). Let me check:

If z = √t, then sinh^{-1}(z) = ln(z + √(z² +1)) = ln(√t + √(t +1)). But in our case, the argument inside the log is √t + √(1 + t). So that's exactly sinh^{-1}(√t). Therefore, ln(√t + √(1 + t)) = sinh^{-1}(√t). Therefore, the logarithm term is sinh^{-1}(√t) where t = x(2 - x). So the integral becomes:

∫₀² x^{1/2} (2 - x)^{-1/2} sinh^{-1}(√[x(2 - x)}) dx.

Hmm, that seems helpful. So substituting t = x(2 - x), but maybe another substitution would be better. Let's see. Let me consider a substitution to simplify the integral. The integrand has x^{1/2} (2 - x)^{-1/2}, which is similar to the form of a Beta function. The Beta function is ∫₀¹ t^{c-1}(1 - t)^{d -1} dt, but here the limits are from 0 to 2. Maybe a substitution to make the interval [0,1]. Let me try substituting x = 2y, so when x=0, y=0; x=2, y=1. Then dx = 2 dy. Then the integral becomes:

∫₀¹ (2y)^{1/2} (2 - 2y)^{-1/2} * sinh^{-1}(√[2y(2 - 2y)}) * 2 dy.

Simplify each term:

(2y)^{1/2} = √2 * y^{1/2}

(2 - 2y)^{-1/2} = (2(1 - y))^{-1/2} = (√2)^{-1} (1 - y)^{-1/2}

Multiply these together: √2 * (√2)^{-1} y^{1/2} (1 - y)^{-1/2} = y^{1/2} (1 - y)^{-1/2}

Then multiply by the 2 from dx: 2 * y^{1/2} (1 - y)^{-1/2}

So the integral becomes:

2 ∫₀¹ y^{1/2} (1 - y)^{-1/2} sinh^{-1}(√[2y(2 - 2y)}) dy.

Wait, let's compute the argument inside sinh^{-1}:

√[2y(2 - 2y)] = √[4y(1 - y)] = 2√[y(1 - y)]

So sinh^{-1}(2√[y(1 - y)}). Therefore, the integral is:

2 ∫₀¹ y^{1/2} (1 - y)^{-1/2} sinh^{-1}(2√[y(1 - y)}) dy.

Hmm, this seems a bit complicated. Maybe another substitution. Let me consider u = y(1 - y). Wait, but that might not help. Alternatively, perhaps a trigonometric substitution. Let me set y = sin²θ. Then dy = 2 sinθ cosθ dθ. When y=0, θ=0; y=1, θ=π/2. Then:

y = sin²θ, 1 - y = cos²θ, √[y(1 - y)] = sinθ cosθ. Then the integral becomes:

2 ∫₀^{π/2} (sin²θ)^{1/2} (cos²θ)^{-1/2} * sinh^{-1}(2 sinθ cosθ) * 2 sinθ cosθ dθ.

Simplify each term:

(sin²θ)^{1/2} = sinθ

(cos²θ)^{-1/2} = 1/cosθ

Multiply these: sinθ / cosθ = tanθ

Then multiply by 2 sinθ cosθ: 2 sinθ cosθ * tanθ = 2 sinθ cosθ * (sinθ / cosθ) = 2 sin²θ

So the integral becomes:

2 * ∫₀^{π/2} 2 sin²θ sinh^{-1}(2 sinθ cosθ) dθ = 4 ∫₀^{π/2} sin²θ sinh^{-1}(sin(2θ)) dθ.

Wait, because 2 sinθ cosθ = sin(2θ). Wait, 2 sinθ cosθ = sin(2θ). So 2θ = 2 sinθ cosθ. Therefore, the argument inside sinh^{-1} is sin(2θ). So sinh^{-1}(sin(2θ)).

Therefore, the integral is 4 ∫₀^{π/2} sin²θ sinh^{-1}(sin(2θ)) dθ.

Hmm, this seems a bit more manageable. Let me see if we can simplify sinh^{-1}(sin(2θ)). The inverse hyperbolic sine of sine. Let's recall that sinh^{-1}(z) = ln(z + √(z² + 1)). So sinh^{-1}(sin(2θ)) = ln(sin(2θ) + √(sin²(2θ) + 1)).

But sin²(2θ) + 1 = 1 + sin²(2θ). Hmm, not sure if that helps. Alternatively, maybe there's a relationship between sinh^{-1}(sin(2θ)) and some angle. Let me think. Suppose we set φ = 2θ. Then when θ goes from 0 to π/2, φ goes from 0 to π. Then the integral becomes:

4 ∫₀^{π} (sin²(φ/2)) * sinh^{-1}(sinφ) * (dφ/2). Wait, θ = φ/2, so dθ = dφ/2. So:

4 * (1/2) ∫₀^{π} sin²(φ/2) sinh^{-1}(sinφ) dφ = 2 ∫₀^{π} sin²(φ/2) sinh^{-1}(sinφ) dφ.

Hmm, not sure if that helps. Alternatively, maybe integrating by parts. Let's consider integrating by parts the original integral. Let me go back to the integral:

4 ∫₀^{π/2} sin²θ sinh^{-1}(sin(2θ)) dθ.

Let me set u = sinh^{-1}(sin(2θ)), dv = 4 sin²θ dθ.

Then du = derivative of sinh^{-1}(sin(2θ)) dθ. Let's compute that. The derivative of sinh^{-1}(z) is 1/√(z² +1) * dz/dθ. So:

du = [1 / √(sin²(2θ) + 1)] * 2 cos(2θ) dθ.

And v = ∫4 sin²θ dθ. Let's compute v:

4 ∫ sin²θ dθ = 4*(θ/2 - sin(2θ)/4) + C = 2θ - sin(2θ) + C.

So integrating by parts:

uv|₀^{π/2} - ∫₀^{π/2} v du.

Compute uv at π/2 and 0:

At θ=π/2: u = sinh^{-1}(sin(π)) = sinh^{-1}(0) = 0. v = 2*(π/2) - sin(π) = π - 0 = π.

So uv = 0 * π = 0.

At θ=0: u = sinh^{-1}(0) = 0, v = 0 - 0 = 0. So uv term is 0 - 0 = 0.

Therefore, the integral becomes - ∫₀^{π/2} v du) = - ∫₀^{π/2} [2θ - sin(2θ)] * [2 cos(2θ) / √(sin²(2θ) + 1)] dθ.

Hmm, this seems more complicated. Maybe this approach isn't the best. Let me think of another substitution.

Wait, let's consider the original substitution. The integral after substitution x = 2y became:

2 ∫₀¹ y^{1/2} (1 - y)^{-1/2} sinh^{-1}(2√[y(1 - y)}) dy.

Alternatively, maybe substitution t = √[y(1 - y)]. Let me set t = √[y(1 - y)}. Then t² = y - y². So y² - y + t² = 0. Solving for y: y = [1 ± √(1 - 4t²)] / 2. Hmm, this might complicate things. Alternatively, maybe substitution z = 2√[y(1 - y)}. Let me set z = 2√[y(1 - y)}. Then z² = 4y(1 - y). So y(1 - y) = z²/4. Let me see if this substitution helps. Then, solving for y: y² - y + z²/4 = 0. Hmm, quadratic in y. Maybe not helpful.

Alternatively, perhaps consider that the integrand has a Beta function form. The term y^{1/2} (1 - y)^{-1/2} is similar to the Beta function integrand. The Beta function B(a,b) = ∫₀¹ y^{a-1} (1 - y)^{b-1} dy. Here, a = 3/2, b = 1/2. But multiplied by sinh^{-1}(2√[y(1 - y)}). So maybe expanding sinh^{-1} as a series and integrating term by term. Let's recall that sinh^{-1}(z) can be expressed as a power series:

sinh^{-1}(z) = z - (1/2)(z³)/3 + (1*3/(2*4))(z^5)/5 - ... for |z| ≤ 1.

But the argument here is 2√[y(1 - y)}. The maximum value of y(1 - y) is 1/4, so √[y(1 - y)} ≤ 1/2, so 2√[y(1 - y)} ≤ 1. Therefore, the argument z = 2√[y(1 - y)} is within the radius of convergence. So maybe expand sinh^{-1}(z) as a power series and integrate term by term.

Let me try that. So:

sinh^{-1}(z) = ∑_{n=0}^∞ (-1)^n (2n)! / (4^n (n!)^2 (2n +1)) z^{2n +1} }, for |z| ≤ 1.

So substituting z = 2√[y(1 - y)}:

sinh^{-1}(2√[y(1 - y)}) = ∑_{n=0}^∞ (-1)^n (2n)! / (4^n (n!)^2 (2n +1)) (2√[y(1 - y)})^{2n +1}

Simplify the term:

(2√[y(1 - y)})^{2n +1} = 2^{2n +1} (y(1 - y))^{n + 1/2}

Therefore, the integral becomes:

2 ∫₀¹ y^{1/2} (1 - y)^{-1/2} * ∑_{n=0}^∞ (-1)^n (2n)! / (4^n (n!)^2 (2n +1)) 2^{2n +1} (y(1 - y))^{n + 1/2} dy

Simplify the constants:

2 * 2^{2n +1} = 2^{2n +2} = 4^{n +1}

So:

∑_{n=0}^∞ (-1)^n (2n)! / (4^n (n!)^2 (2n +1)) * 4^{n +1} ∫₀¹ y^{1/2} (1 - y)^{-1/2} (y(1 - y))^{n + 1/2} dy

Simplify the constants:

4^{n +1} / 4^n = 4

So:

4 ∑_{n=0}^∞ (-1)^n (2n)! / (n!)^2 (2n +1) ∫₀¹ y^{1/2} (1 - y)^{-1/2} (y(1 - y))^{n + 1/2} dy

Combine the exponents in the integrand:

y^{1/2} * (y(1 - y))^{n + 1/2} = y^{1/2 + n + 1/2} (1 - y)^{n + 1/2} = y^{n +1} (1 - y)^{n + 1/2 -1/2} = y^{n +1} (1 - y)^n

Wait, let me check:

Original exponents:

y^{1/2} * [y^{n + 1/2} (1 - y)^{n + 1/2}] = y^{1/2 + n + 1/2} (1 - y)^{ -1/2 + n + 1/2}

Wait, no. Wait, the term (y(1 - y))^{n + 1/2} is y^{n + 1/2} (1 - y)^{n + 1/2}

So multiplying by y^{1/2} (1 - y)^{-1/2} gives:

y^{1/2 + n + 1/2} (1 - y)^{-1/2 + n + 1/2} = y^{n +1} (1 - y)^n

Yes, because 1/2 + n +1/2 = n +1, and -1/2 + n +1/2 = n.

Therefore, the integral becomes:

4 ∑_{n=0}^∞ (-1)^n (2n)! / (n!)^2 (2n +1) ∫₀¹ y^{n +1} (1 - y)^n dy

The integral ∫₀¹ y^{n +1} (1 - y)^n dy is the Beta function B(n +2, n +1) = Γ(n +2)Γ(n +1)/Γ(2n +3). But Γ(n +2) = (n +1)!, Γ(n +1) = n!, Γ(2n +3) = (2n +2)! So:

B(n +2, n +1) = (n +1)! n! / (2n +2)! )

But (2n +2)! = (2n +2)(2n +1)! )

So:

B(n +2, n +1) = (n +1)! n! / [ (2n +2)(2n +1)! ) ] = [n! (n +1)! ) ] / [ 2(n +1)(2n +1)! ) ] = [n! / (2(2n +1)! ) ]

Wait, let's compute it step by step:

Γ(n +2) = (n +1)!

Γ(n +1) = n!

Γ(2n +3) = (2n +2)(2n +1)!

Therefore,

B(n +2, n +1) = (n +1)! n! / [ (2n +2)(2n +1)! ) ] = [ (n +1) n! n! ] / [ 2(n +1)(2n +1)! ) ] = [ n! n! ] / [ 2 (2n +1)! ) ]

So the integral becomes:

4 ∑_{n=0}^∞ (-1)^n (2n)! / (n!^2 (2n +1)) * [ n! n! / (2 (2n +1)! ) ]

Simplify the terms:

(2n)! / (n!^2) is the central binomial coefficient, which is (2n choose n). Then:

4 * [ (2n)! / (n!^2 (2n +1)) ] * [ n!^2 / (2 (2n +1)! ) ] = 4 * (2n)! / (2 (2n +1) (2n +1)! )) )

But (2n +1)! = (2n +1)(2n)! So:

= 4 * (2n)! / (2 (2n +1) (2n +1)(2n)! )) ) = 4 / [ 2 (2n +1)^2 ] = 2 / (2n +1)^2

Therefore, the entire sum becomes:

4 ∑_{n=0}^∞ (-1)^n [ 2 / (2n +1)^2 ] = 8 ∑_{n=0}^∞ (-1)^n / (2n +1)^2

Wait, wait, let me check again:

Wait, the expression after substituting the Beta function:

4 * [ (2n)! / (n!^2 (2n +1)) ] * [ n!^2 / (2 (2n +1)! ) ] = 4 * (2n)! * n!^2 / (n!^2 (2n +1) * 2 (2n +1)! )) )

Simplify numerator and denominator:

4 / (2 (2n +1)) * (2n)! / (2n +1)! )

But (2n +1)! = (2n +1)(2n)! So:

4 / (2 (2n +1)) * 1 / (2n +1) ) = 4 / (2 (2n +1)^2 ) = 2 / (2n +1)^2

Therefore, the sum is:

2 ∑_{n=0}^∞ (-1)^n / (2n +1)^2

But wait, the original sum had a factor of 4 multiplied by the sum over n of (-1)^n (2n)! / (n!^2 (2n +1)) * B(n +2, n +1). Which we simplified to 2 ∑_{n=0}^∞ (-1)^n / (2n +1)^2.

Therefore, the integral equals 2 times the sum over n from 0 to ∞ of (-1)^n / (2n +1)^2.

But this sum is known. The sum ∑_{n=0}^∞ (-1)^n / (2n +1)^2 is Catalan's constant, denoted by G. However, Catalan's constant is defined as G = ∑_{n=0}^∞ (-1)^n / (2n +1)^2 ≈ 0.9159655942...

Therefore, the integral equals 2G. So the exact answer is 2G, and the numerical value is approximately 2 * 0.9159655942 ≈ 1.8319311884.

Wait, but let me confirm this. The sum ∑_{n=0}^∞ (-1)^n/(2n+1)^2 is indeed Catalan's constant. So the integral is 2G. Therefore, the exact answer is 2G, and the numerical approximation is approximately 1.8319311884.

But let me check if there's any mistake in the steps. Let's recap:

We started with substitution x = 2y, transformed the integral into a form involving sinh^{-1}(2√[y(1 - y)}), expanded sinh^{-1} as a power series, integrated term by term using Beta functions, and found that the integral reduces to 2G. This seems correct.

Alternatively, maybe there's a smarter substitution. Let me think. The original integrand is x^{1/2} (2 - x)^{-1/2} ln(...). Let me consider substitution t = x/(2 - x). Then x = 2t/(1 + t), dx = 2/(1 + t)^2 dt. When x=0, t=0; x=2, t approaches infinity. Hmm, but integrating from 0 to infinity might complicate things. Let's try:

Let t = x/(2 - x). Then x = 2t/(1 + t), 2 - x = 2/(1 + t). Then:

x^{1/2} = (2t/(1 + t))^{1/2} = √(2t)/(1 + t)^{1/2}

(2 - x)^{-1/2} = (2/(1 + t))^{-1/2} = (1 + t)^{1/2}/√2

dx = 2/(1 + t)^2 dt

So the integrand becomes:

√(2t)/(1 + t)^{1/2} * (1 + t)^{1/2}/√2 * ln(...) * 2/(1 + t)^2 dt

Simplify:

√(2t)/√2 = √t

(1 + t)^{1/2} cancels with (1 + t)^{1/2}

So we have √t * 2/(1 + t)^2 dt

Now, the logarithm term:

ln(√[x(2 - x)} + √[1 + x(2 - x)})

Substitute x = 2t/(1 + t), 2 - x = 2/(1 + t)

x(2 - x) = [2t/(1 + t)] * [2/(1 + t)] = 4t/(1 + t)^2

So √[x(2 - x)} = 2√t/(1 + t)

Then 1 + x(2 - x) = 1 + 4t/(1 + t)^2 = [ (1 + t)^2 + 4t ] / (1 + t)^2 = (1 + 2t + t² + 4t) / (1 + t)^2 = (1 + 6t + t²)/(1 + t)^2. Wait, no:

Wait, 1 + x(2 - x) = 1 + 4t/(1 + t)^2. Let me compute that:

= [ (1 + t)^2 + 4t ] / (1 + t)^2

= (1 + 2t + t² + 4t) / (1 + t)^2

= (1 + 6t + t²) / (1 + t)^2. Wait, that's not correct. Wait, 1 + 4t/(1 + t)^2. Let me compute numerator:

(1 + t)^2 + 4t = 1 + 2t + t² + 4t = 1 + 6t + t². So yes.

Then √[1 + x(2 - x)} = √(1 + 6t + t²)/(1 + t)

Therefore, the argument of the logarithm is:

2√t/(1 + t) + √(1 + 6t + t²)/(1 + t) = [2√t + √(1 + 6t + t²)] / (1 + t)

Hmm, not sure if this helps. Let me check if 1 + 6t + t² can be expressed as a square. Let's see:

Suppose 1 + 6t + t² = (t + a)^2 + b. Expanding: t² + 2at + a² + b. Comparing coefficients:

2a = 6 => a = 3. Then a² + b = 1 + b = 1 => 9 + b =1 => b= -8. So 1 +6t + t² = (t +3)^2 -8. Not a perfect square. Alternatively, maybe another approach.

Alternatively, perhaps the expression inside the log can be simplified. Let me compute:

2√t + √(1 +6t + t²). Let me set s = √t. Then t = s², dt = 2s ds. Then the expression becomes 2s + √(1 +6s² + s^4). Hmm, not sure. Alternatively, maybe factor 1 +6t +t². The discriminant is 36 -4*1*1=32, so roots are (-6 ±√32)/2 = (-6 ±4√2)/2 = -3 ±2√2. So 1 +6t +t² = (t +3 -2√2)(t +3 +2√2). Not helpful.

Alternatively, maybe this substitution isn't helpful. Let's go back. The integral after substitution t = x/(2 -x) becomes:

∫₀^∞ √t * 2/(1 + t)^2 * ln( [2√t + √(1 +6t + t²)] / (1 + t) ) dt

Hmm, not sure. Maybe this isn't the right path. Let's return to the previous result where the integral equals 2G. Since we arrived there through power series expansion and term-by-term integration, and the steps seem correct, perhaps that's the answer.

Catalan's constant G is a known constant, approximately 0.915965594177219... So multiplying by 2 gives approximately 1.831931188354438... Rounded to 10 decimal places, that's 1.8319311884.

Therefore, the exact answer is 2G, which can be written in LaTeX as 2\mathbf{G}, but since it's a standard constant, it's usually denoted as G. However, since the problem asks for the exact answer, and the integral evaluates to 2 times Catalan's constant, the exact answer is 2G. However, if the problem expects a closed-form in terms of known constants, then 2G is the exact answer. If not, then perhaps another form. But given the steps lead us to 2G, and G is a recognized mathematical constant, that's the exact answer.

Therefore, the final answer is 2G, and numerically approximately 1.8319311884.
</think>

{"answer": "2\\mathbf{G}", "numerical_answer": "1.8319311884"}