Let's compute the integral:
\[
I = \int_0^\infty \frac{\tanh(x)}{e^x} \, dx
\]

### 1. **Express \(\tanh(x)\) in terms of exponentials:**
\[
\tanh(x) = \frac{e^{x}-e^{-x}}{e^{x}+e^{-x}}
\]
So,
\[
\frac{\tanh(x)}{e^x} = \frac{e^{x} - e^{-x}}{e^{x}+e^{-x}} \cdot \frac{1}{e^x}
= \frac{1 - e^{-2x}}{e^{x}+e^{-x}}
\]

But let's rewrite \(\tanh(x)\):
\[
\tanh(x) = 1 - \frac{2}{e^{2x}+1}
\]
So,
\[
\frac{\tanh(x)}{e^x} = \frac{1}{e^x} - \frac{2}{e^x(e^{2x}+1)}
\]

### 2. **Write the integral as two simpler integrals:**
\[
I = \int_0^\infty \frac{1}{e^x} dx - 2\int_0^\infty \frac{dx}{e^x(e^{2x}+1)}
= I_1 - 2I_2
\]
where,
\[
I_1 = \int_0^\infty e^{-x} dx = 1
\]
\[
I_2 = \int_0^\infty \frac{dx}{e^x(e^{2x}+1)}
\]

### 3. **Evaluate \(I_2\) using substitution:**

Let \(u = e^x\) with \(du = e^x dx\), thus \(dx = \frac{du}{u}\) and when \(x = 0\), \(u = 1\); \(x \to \infty \implies u \to \infty\).
So,
\[
I_2 = \int_{x=0}^{x=\infty} \frac{dx}{e^x(e^{2x}+1)}
= \int_{u=1}^{u=\infty} \frac{1}{u \left(u^2+1\right)} \frac{du}{u}
= \int_{u=1}^{u=\infty} \frac{du}{u^2(u^2+1)}
\]

Decompose:
\[
\frac{1}{u^2(u^2+1)} = \frac{A}{u} + \frac{B}{u^2} + \frac{Cu + D}{u^2+1}
\]

Multiply both sides by \(u^2(u^2+1)\):
\[
1 = A u(u^2+1) + B(u^2+1) + (Cu+D)u^2
= A u^3 + A u + Bu^2 + B + C u^3 + D u^2
\]
Group terms:
\[
u^3: (A+C)
u^2: (B+D)
u^1: A
u^0: B
\]
Set equal to 1, so:
\[
A + C = 0 \\
B + D = 0 \\
A = 0 \\
B = 1
\]
So \(A=0\), \(B=1\). From \(A + C=0\), \(C=0\), from \(B+D=0\), \(D=-1\).

Therefore,
\[
\frac{1}{u^2(u^2+1)} = \frac{1}{u^2} - \frac{1}{u^2+1}
\]

So,
\[
I_2 = \int_1^\infty \left( \frac{1}{u^2} - \frac{1}{u^2+1} \right) du
\]

Now, integrate:
\[
\int_1^\infty \frac{1}{u^2} du = \left[ -\frac{1}{u} \right]_{1}^{\infty} = 0 - (-1) = 1
\]
\[
\int_1^\infty \frac{1}{u^2+1} du = \left[ \arctan(u) \right]_{1}^{\infty}
= \frac{\pi}{2} - \frac{\pi}{4} = \frac{\pi}{4}
\]

Thus,
\[
I_2 = 1 - \frac{\pi}{4}
\]
So,
\[
I = I_1 - 2I_2 = 1 - 2 \left( 1 - \frac{\pi}{4} \right ) = 1 - 2 + \frac{\pi}{2} = -1 + \frac{\pi}{2}
\]

### 4. **Numerical approximation:**
\[
I = -1 + \frac{\pi}{2} \approx -1 + 1.5707963268 = 0.5707963268
\]

### Final Answer
```json
{"answer": "-1+\\frac{\\pi}{2}", "numerical_answer": "0.5707963268"}
```