<think>
Okay, let's tackle this integral: ∫₀¹ [ln(x + x⁻¹)] / (x + x⁻¹) dx. Hmm, that looks a bit complicated. First, I need to simplify the expression if possible. The integrand is [ln(x + 1/x)] divided by (x + 1/x). Let me see if substituting t = x + 1/x would help. But before that, maybe a substitution to make the integral more manageable.

Wait, the limits are from 0 to 1. When x approaches 0, x⁻¹ becomes very large, so x + x⁻¹ tends to infinity. At x=1, x + x⁻¹ is 2. So the integrand at x=1 is ln(2)/2, which is finite. But near x=0, the integrand behaves like ln(1/x)/(1/x) = x ln(1/x) = -x ln x, which tends to 0 as x approaches 0. So the integral should converge.

Maybe substitution: Let’s try t = x - 1/x. Wait, not sure. Alternatively, let me consider substituting u = x². Let’s see. Let u = x², then du = 2x dx. Hmm, not sure if that helps. Alternatively, maybe substitution to exploit symmetry. Let’s consider substituting x = 1/t. Let’s try that. Let x = 1/t, so when x approaches 0, t approaches infinity, and when x=1, t=1. Then dx = -1/t² dt. Let's compute the integral:

Original integral from 0 to 1 becomes integral from t=∞ to t=1 of [ln(1/t + t)] / (1/t + t) * (-1/t²) dt. Changing the limits to 1 to ∞ and flipping the sign, we get integral from 1 to ∞ of [ln(t + 1/t)] / (t + 1/t) * (1/t²) dt.

But the integrand here is [ln(t + 1/t)] / (t + 1/t) * (1/t²). Let me see if this is similar to the original integrand. The original integrand was [ln(x + 1/x)] / (x + 1/x) dx. If we add the original integral I and the transformed integral after substitution, maybe we can get something.

Let me denote I = ∫₀¹ [ln(x + 1/x)] / (x + 1/x) dx. Then after substitution, the transformed integral is ∫₁^∞ [ln(t + 1/t)] / (t + 1/t) * (1/t²) dt. Let me call this integral J. So I + J = ∫₀¹ ... dx + ∫₁^∞ ... dt. But maybe there's a way to relate I and J. Let me compute J. Let's write J as ∫₁^∞ [ln(t + 1/t)] / (t + 1/t) * (1/t²) dt. Let me make a substitution in J: let u = 1/t. Then when t=1, u=1; t=∞, u=0. Then du = -1/t² dt, so dt = -t² du. But substituting u=1/t, t=1/u, so J becomes ∫₀¹ [ln(1/u) + u] / (1/u + u) * (1/(1/u)²) * (-u² du). Wait, this might get messy. Let me compute step by step.

Wait, substitution u = 1/t. Then t = 1/u, dt = -1/u² du. So J becomes:

∫_{u=1}^{u=0} [ln(1/u + u)] / (1/u + u) * (1/(1/u)^2) * (-1/u²) du

Simplify the terms:

First, 1/(1/u + u) = u/(1 + u²). Then, 1/(1/u)^2 = u². Then, the integrand becomes:

[ln(1/u + u)] * [u/(1 + u²)] * u²] * (1/u²) du

Wait, let's do it step by step. The original integrand of J is [ln(t + 1/t)] / (t + 1/t) * (1/t²). Substituting t = 1/u, so:

ln(1/u + u) / (1/u + u) * (1/(1/u)^2) * (-1/u²) du

First, 1/u + u = (1 + u²)/u. So denominator is (1 + u²)/u. Then, the ln term is ln((1 + u²)/u). The 1/t² term is u². So putting it all together:

[ln((1 + u²)/u) / ((1 + u²)/u)] * u² * (-1/u²) du

Simplify:

The denominator (1 + u²)/u becomes u/(1 + u²) when inverted. So:

ln((1 + u²)/u) * [u/(1 + u²)] * u² * (-1/u²) du

Wait, perhaps I made a miscalculation here. Let me re-express:

Original integrand after substitution:

[ln((1/u) + u)] / [(1/u) + u] * (1/(1/u)^2) * (-1/u²) du

First, (1/u) + u = (1 + u²)/u. So denominator is (1 + u²)/u. Then 1/(1/u)^2 is u². So:

[ln((1 + u²)/u)] / [(1 + u²)/u] * u² * (-1/u²) du

Simplify term by term:

The first part: [ln((1 + u²)/u)] / [(1 + u²)/u] = [ln((1 + u²)/u) * u]/(1 + u²)

Multiply by u²: [ln((1 + u²)/u) * u]/(1 + u²) * u² = [ln((1 + u²)/u) * u³]/(1 + u²)

Multiply by (-1/u²): [ln((1 + u²)/u) * u³]/(1 + u²) * (-1/u²) = - [ln((1 + u²)/u) * u]/(1 + u²) du

So J becomes ∫_{u=1}^{0} - [ln((1 + u²)/u) * u]/(1 + u²) du. Changing the limits back to 0 to 1 and removing the negative sign:

J = ∫₀¹ [ln((1 + u²)/u) * u]/(1 + u²) du

But (1 + u²)/u = u + 1/u, so ln((1 + u²)/u) = ln(u + 1/u). Therefore, J = ∫₀¹ [ln(u + 1/u) * u]/(1 + u²) du

Compare this with the original integral I = ∫₀¹ [ln(x + 1/x)] / (x + 1/x) dx. So J is similar but with an extra factor of u in the numerator and denominator (1 + u²). Let me write both integrals:

I = ∫₀¹ [ln(x + 1/x)] / (x + 1/x) dx

J = ∫₀¹ [ln(x + 1/x) * x]/(1 + x²) dx

So if we add I and J:

I + J = ∫₀¹ [ln(x + 1/x)] / (x + 1/x) + [ln(x + 1/x) * x]/(1 + x²) dx

Factor out ln(x + 1/x):

I + J = ∫₀¹ ln(x + 1/x) [1/(x + 1/x) + x/(1 + x²)] dx

Let me compute the expression inside the brackets:

1/(x + 1/x) + x/(1 + x²) = [1/( (x² + 1)/x ) ] + x/(1 + x²) = x/(x² + 1) + x/(x² + 1) = 2x/(x² + 1)

So I + J = ∫₀¹ ln(x + 1/x) * [2x/(x² + 1)] dx

Hmm, interesting. So I + J = 2 ∫₀¹ [x ln(x + 1/x)] / (x² + 1) dx

But wait, can we relate this to J? Let me see. Alternatively, maybe we can find a substitution that connects I and J. Let me think.

Alternatively, let's consider that x + 1/x = t. Let’s try substitution t = x + 1/x. Then dt/dx = 1 - 1/x². Hmm, but integrating with respect to t might complicate things. Alternatively, maybe another substitution.

Wait, let's consider splitting the logarithm: ln(x + 1/x) = ln(x² + 1) - ln x. So:

I = ∫₀¹ [ln(x² + 1) - ln x] / (x + 1/x) dx

Which can be written as:

I = ∫₀¹ [ln(x² + 1) - ln x] * x / (x² + 1) dx

Because 1/(x + 1/x) = x/(x² + 1). So:

I = ∫₀¹ [ln(x² + 1) - ln x] * x / (x² + 1) dx

Split into two integrals:

I = ∫₀¹ [x ln(x² + 1)] / (x² + 1) dx - ∫₀¹ [x ln x] / (x² + 1) dx

Let’s handle the first integral: Let’s set u = x² + 1, then du = 2x dx. So x dx = du/2. Then the first integral becomes:

∫ [ln u] / u * (du/2) from u=1 to u=2. So (1/2) ∫₁² (ln u)/u du = (1/2) * [ (ln u)^2 / 2 ] from 1 to 2 = (1/4)[ (ln 2)^2 - 0 ] = (ln 2)^2 / 4? Wait, no. Wait, integral of (ln u)/u du is (ln u)^2 / 2. So yes, (1/2) * [ (ln 2)^2 / 2 - (ln 1)^2 / 2 ] = (1/4)(ln 2)^2.

So first integral is (ln 2)^2 / 4? Wait, no. Wait, step by step:

First integral: ∫₀¹ [x ln(x² + 1)] / (x² + 1) dx

Let u = x² + 1, du = 2x dx => x dx = du/2. When x=0, u=1; x=1, u=2.

So integral becomes ∫₁² [ln u / u] * (du/2) = (1/2) ∫₁² (ln u)/u du

Integral of (ln u)/u du is (ln u)^2 / 2. So evaluated from 1 to 2:

(1/2) * [ (ln 2)^2 / 2 - (ln 1)^2 / 2 ] = (1/2) * [ ( (ln 2)^2 ) / 2 - 0 ] = (ln 2)^2 / 4.

So first integral is (ln 2)^2 / 4.

Now, the second integral: ∫₀¹ [x ln x] / (x² + 1) dx

Let’s consider substitution. Let’s set t = x², so dt = 2x dx, x dx = dt/2. Then the integral becomes:

∫₀¹ [ln x] * x / (x² + 1) dx = ∫₀¹ [ln sqrt(t)] / (t + 1) * (dt/2)

Because x = sqrt(t), so ln x = (1/2) ln t. So:

= (1/2) ∫₀¹ [ (1/2) ln t ) / (t + 1) ] dt

Wait, no. Wait, x = sqrt(t), so ln x = (1/2) ln t. So:

= ∫₀¹ [ (1/2) ln t ] / (t + 1) * (dt/2) = (1/4) ∫₀¹ (ln t)/(t + 1) dt

So the second integral is (1/4) ∫₀¹ (ln t)/(t + 1) dt

Hmm, the integral ∫₀¹ (ln t)/(t + 1) dt is a standard integral. Let me recall that ∫₀¹ (ln t)/(1 + t) dt = -π²/12. Wait, how?

Alternatively, consider expanding 1/(1 + t) as a power series. For t in (0,1), 1/(1 + t) = Σ (-1)^n t^n from n=0 to ∞. Then:

∫₀¹ (ln t) Σ (-1)^n t^n dt = Σ (-1)^n ∫₀¹ t^n ln t dt

Integrate term by term. The integral ∫ t^n ln t dt can be integrated by parts. Let u = ln t, dv = t^n dt. Then du = (1/t) dt, v = t^{n+1}/(n+1). So:

∫ t^n ln t dt = (t^{n+1}/(n+1)) ln t - ∫ t^{n+1}/(n+1) * (1/t) dt = (t^{n+1} ln t)/(n+1) - 1/(n+1) ∫ t^n dt = (t^{n+1} ln t)/(n+1) - t^{n+1}/ (n+1)^2 + C

Evaluated from 0 to 1. At t=1, the first term is 0 (since ln 1=0), and the second term is -1/(n+1)^2. At t=0, t^{n+1} ln t approaches 0 (since t^{n+1} approaches 0 and ln t approaches -infty, but the product tends to 0), and t^{n+1}/(n+1)^2 also approaches 0. So the integral from 0 to1 is -1/(n+1)^2.

Therefore, the sum becomes Σ (-1)^n * (-1)/(n+1)^2) = Σ (-1)^{n+1}/(n+1)^2. Let’s adjust the index: let m = n + 1, so when n=0, m=1. Then the sum becomes Σ_{m=1}^∞ (-1)^m / m². This is known as the Dirichlet eta function at 2: η(2) = (1 - 2^{1 - 2}) ζ(2) = (1 - 1/2) π²/6 = π²/12. But since the sum is Σ (-1)^m / m² from m=1 to ∞ = -η(2) = -π²/12. Wait, let me check:

Wait, η(s) = Σ_{n=1}^∞ (-1)^{n+1}/n^s. So η(2) = Σ_{n=1}^∞ (-1)^{n+1}/n² = π²/12. Therefore, our sum Σ_{m=1}^∞ (-1)^m / m² = -η(2) = -π²/12. Therefore, the integral ∫₀¹ (ln t)/(1 + t) dt = -π²/12.

Therefore, the second integral is (1/4) * (-π²/12) = -π²/(48).

So putting it all together, the original integral I is:

I = (ln 2)^2 / 4 - (-π²/48) = (ln 2)^2 / 4 + π²/48? Wait, no. Wait, the first integral was (ln 2)^2 / 4? Wait, no:

Wait, first integral was (ln 2)^2 / 4. Second integral was -π²/(48). So I = (ln 2)^2 / 4 - ( -π²/48 )? Wait, no. Wait, the second integral is subtracted, so:

I = (ln 2)^2 / 4 - [ -π²/(48) ] = (ln 2)^2 / 4 + π²/48. Wait, no:

Wait, the second integral is ∫ [x ln x]/(x² +1) dx = (1/4) ∫₀¹ (ln t)/(t +1) dt = (1/4)( -π²/12 ) = -π²/(48). So I = first integral - second integral = (ln 2)^2 /4 - ( -π²/48 )? Wait, no. Wait, the original split was:

I = first integral - second integral. The first integral is (ln 2)^2 /4. The second integral is -π²/48. So I = (ln 2)^2 /4 - ( -π²/48 )? Wait, no. Wait, the second integral is negative. Let me re-express:

I = [ (ln 2)^2 /4 ] - [ -π²/48 ] = (ln 2)^2 /4 + π²/48.

Wait, no. Wait, the second integral is ∫ [x ln x]/(x² +1) dx = (1/4)( -π²/12 ) = -π²/(48). So when we subtract this integral, it's minus a negative, so:

I = (ln 2)^2 /4 - ( -π²/48 ) = (ln 2)^2 /4 + π²/48.

So I = (ln 2)^2 /4 + π²/48.

But wait, let me check the signs again. The original split was:

I = ∫ [x ln(x² +1)]/(x² +1) dx - ∫ [x ln x]/(x² +1) dx

First integral is positive (ln 2)^2 /4. Second integral is -π²/48. So I = (ln 2)^2 /4 - (-π²/48) = (ln 2)^2 /4 + π²/48.

Yes, that's correct.

So the exact value is (ln 2)/4 + π²/48.

Wait, but let me check the calculation again. Because when I split the original integral into two parts, the first integral was (x ln(x² +1))/(x² +1) dx, which became (ln 2)^2 /4. The second integral was - ∫ (x ln x)/(x² +1) dx, which was - [ -π²/48 ] = + π²/48. So yes, I = (ln 2)^2 /4 + π²/48.

Alternatively, combining the terms:

Let me compute (ln 2)^2 /4 + π²/48. To check if this can be simplified further. Maybe factor out 1/48:

= (12 (ln 2)^2 + π²)/48.

But not sure if that's necessary. So the exact answer is (ln 2)^2 /4 + π²/48.

Now, let's compute the numerical approximation. Let's compute each term:

First, ln 2 ≈ 0.69314718056. So (ln 2)^2 ≈ (0.69314718056)^2 ≈ 0.480453013918. Divided by 4: 0.480453013918 /4 ≈ 0.1201132534795.

Next, π² ≈ 9.8696044011. Divided by 48: 9.8696044011 /48 ≈ 0.205616758356.

Adding them together: 0.1201132534795 + 0.205616758356 ≈ 0.3257300118355. Rounded to 10 decimal places: 0.3257300118.

Wait, but let me check with more precise calculations.

First, compute ln(2):

ln(2) ≈ 0.69314718055994530941723212145818

(ln 2)^2 ≈ 0.6931471805599453^2 ≈ 0.4804530139182016

0.4804530139182016 /4 = 0.1201132534795504

π² ≈ 9.869604401089358

9.869604401089358 /48 ≈ 0.2056167583560283

Sum: 0.1201132534795504 + 0.2056167583560283 ≈ 0.3257300118355787

Rounded to 10 decimal places: 0.3257300118

But let me check with more precise calculation:

0.1201132534795504 + 0.2056167583560283 = 0.3257300118355787

Yes, so approximately 0.3257300118.

Therefore, the exact answer is (ln 2)^2 /4 + π²/48, and the numerical approximation is approximately 0.3257300118.

But wait, let me check if there's a simpler form. Let me see:

(ln 2)^2 /4 + π²/48. Alternatively, factor out 1/48:

= (12 (ln 2)^2 + π²)/48. Not sure if that's simpler. Alternatively, maybe there's a different expression. Let me think if there's another approach.

Alternatively, going back to the original substitution where I + J = 2 ∫₀¹ [x ln(x + 1/x)] / (x² +1) dx. But we found that I = (ln 2)^2 /4 + π²/48. But maybe there's another way to express this. However, given the steps we took, this seems to be the correct exact answer.

Therefore, the final answer is (ln 2)^2 /4 + π²/48, and the approximation is approximately 0.3257300118.
</think>

{"answer": "\\frac{(\\ln 2)^2}{4} + \\frac{\\pi^2}{48}", "numerical_answer": 0.3257300118}