Let's compute the integral:
\[
I = \int_{0}^{1} \arcsin\left(0.5 \sqrt{x(1-x)}\right) dx
\]

### Step 1: Substitution

Let us use the substitution \(x = \sin^2 \theta\), where as \(x\) goes from \(0\) to \(1\), \(\theta\) goes from \(0\) to \(\pi/2\).

Compute:
\[
dx = 2\sin\theta \cos\theta d\theta = \sin(2\theta) d\theta
\]
\[
1-x = 1 - \sin^2\theta = \cos^2\theta
\]
\[
\sqrt{x(1-x)} = \sqrt{\sin^2\theta \cos^2\theta} = \sin\theta \cos\theta
\]

So the argument of \(\arcsin\) becomes:
\[
0.5 \sqrt{x(1-x)} = 0.5 \sin\theta \cos\theta = 0.25 \sin 2\theta
\]

Thus, the integral becomes:
\[
I = \int_{0}^{\pi/2} \arcsin(0.25\sin 2\theta) \cdot \sin 2\theta d\theta
\]

### Step 2: Let \(u = 2\theta\)

Now set \(u = 2\theta\), so as \(\theta\) goes from \(0\) to \(\pi/2\), \(u\) goes from \(0\) to \(\pi\).

Thus,
\[
\sin 2\theta = \sin u
\]
\[
d\theta = du/2
\]

So the integral becomes:
\[
I = \int_{u=0}^{u=\pi} \arcsin(0.25\sin u) \cdot \sin u \cdot \frac{du}{2}
= \frac{1}{2} \int_{0}^{\pi} \arcsin(0.25 \sin u) \sin u du
\]

### Step 3: Compute the Integral

Let us write:
\[
J = \int_{0}^{\pi} \arcsin(a \sin u) \sin u du \quad \text{with} \ a = 0.25
\]

But, more generally, consider:
\[
J(a) = \int_{0}^{\pi} \arcsin(a \sin u) \sin u du
\]

Let us try to find an analytic expression for \(J(a)\):

#### Integrating by Parts

Let:
\[
f(u) = \arcsin(a \sin u), \quad g'(u) = \sin u
\]
\[
\text{Let } g(u) = -\cos u
\]

Then,
\[
J(a) = \left[ f(u) g(u) \right]_0^{\pi} - \int_0^\pi f'(u) g(u) du
\]
\[
= \left[ \arcsin(a \sin u)(-\cos u) \right]_0^\pi + \int_0^\pi f'(u)\cos u du
\]

The boundary term:
\[
\sin 0 = 0,\, \sin \pi = 0 \implies f(0) = f(\pi) = 0
\implies \arcsin(a \sin u)(-\cos u)\Big|_0^\pi = 0
\]

So,
\[
J(a) = \int_{0}^{\pi} f'(u) \cos u du
\]
\[
f'(u) = \frac{a\cos u}{\sqrt{1 - (a\sin u)^2}}
\]
So,
\[
J(a) = \int_0^\pi \frac{a \cos^2 u}{\sqrt{1 - a^2 \sin^2 u}} du
\]

Recall \(\cos^2 u = 1 - \sin^2 u\), so:
\[
J(a) = a \int_0^\pi \frac{1 - \sin^2 u}{\sqrt{1 - a^2 \sin^2 u}} du
= a\int_0^\pi \frac{du}{\sqrt{1 - a^2 \sin^2 u}} - a \int_0^\pi \frac{\sin^2 u du}{\sqrt{1 - a^2 \sin^2 u}}
\]

Let’s make the substitution for both integrals.

First, notice:
\[
\int_0^\pi \frac{du}{\sqrt{1 - k^2 \sin^2 u}} = 2K(k)
\]
where \(K(k)\) is the complete elliptic integral of the first kind.

Also,
\[
\int_0^\pi \frac{\sin^2 u du}{\sqrt{1 - k^2 \sin^2 u}}
\]
There’s a standard integral (Byrd & Friedman, formula 218.13):
\[
\int_0^\pi \frac{\sin^2 u\, du}{\sqrt{1 - k^2 \sin^2 u}} = \frac{2}{k^2}\left[K(k) - E(k)\right]
\]
where \(E(k)\) is the complete elliptic integral of the second kind.

So, plugging in \(a = 0.25\) (so \(k = 0.25\)), we have:
\[
J(0.25) = 0.25 \left[2K(0.25) - 2\frac{K(0.25) - E(0.25)}{(0.25)^2} \right]
= 0.5 K(0.25) - 2 \frac{K(0.25) - E(0.25)}{0.25^2}
\]
Since \(0.25^2 = 0.0625\) and \(1/0.0625 = 16\):
\[
J(0.25) = 0.5 K(0.25) - 32 \left[K(0.25) - E(0.25)\right]
\]

Recall,
\[
I = \frac{1}{2} J(0.25)
\]
Therefore,
\[
I = \frac{1}{2} \left[0.5 K(0.25) - 32 \left(K(0.25) - E(0.25)\right)\right]
\]
\[
I = 0.25 K(0.25) - 16 \left(K(0.25) - E(0.25)\right)
\]

#### Final Exact Answer

\[
I = 0.25 K(0.25) - 16 \left[K(0.25) - E(0.25)\right]
\]

We can write this as:
\[
I = -15.75\, K(0.25) + 16\, E(0.25)
\]

### Step 4: Numerical Approximation

Let’s numerically evaluate:
- \(K(0.25)\)
- \(E(0.25)\)

From standard tables or computational tools,

- \(K(0.25) \approx 1.612441348720219\)
- \(E(0.25) \approx 1.530757636897763\)

Thus,
\[
I = -15.75 \times 1.612441348720219 + 16 \times 1.530757636897763
\]
Compute:

- \( -15.75 \times 1.612441348720219 \approx -25.41495124185345 \)
- \( 16 \times 1.530757636897763 \approx 24.49212219036421 \)

So,

\[
I \approx -25.41495124185345 + 24.49212219036421 = -0.92282905148924
\]

Rounded to 10 decimal places:

\[
I \approx -0.9228290515
\]

### Final Answer (in JSON format)

```json
{"answer": "-15.75\\, K(0.25) + 16\\, E(0.25)", "numerical_answer": "-0.9228290515"}
```