

To solve the definite integral \(\int_{-1}^1 \frac{\cos x}{1 + e^{-\frac{1}{x}}}\, dx\), we use symmetry and substitution.

### Step 1: Substitution \(x \to -t\)
Let \(t = -x\), so \(dx = -dt\). When \(x = -1\), \(t = 1\), and when \(x = 1\), \(t = -1\). The integral becomes:
\[
I = \int_{-1}^1 \frac{\cos x}{1 + e^{-\frac{1}{x}}}\, dx = \int_{1}^{-1} \frac{\cos(-t)}{1 + e^{-\frac{1}{-t}}}\, (-dt)
\]
Reversing the limits and simplifying \(\cos(-t) = \cos t\) and \(e^{-\frac{1}{-t}} = e^{\frac{1}{t}}\), we get:
\[
I = \int_{-1}^1 \frac{\cos t}{1 + e^{\frac{1}{t}}}\, dt
\]
Since \(t\) is a dummy variable, we rewrite this as:
\[
I = \int_{-1}^1 \frac{\cos x}{1 + e^{\frac{1}{x}}}\, dx
\]

### Step 2: Adding the original and substituted integrals
Add the original integral \(I\) and the substituted integral \(I\):
\[
2I = \int_{-1}^1 \left( \frac{\cos x}{1 + e^{-\frac{1}{x}}} + \frac{\cos x}{1 + e^{\frac{1}{x}}} \right) dx
\]
Simplify the integrand by combining the fractions. Let \(a = e^{\frac{1}{x}}\), so \(e^{-\frac{1}{x}} = \frac{1}{a}\). Then:
\[
\frac{1}{1 + e^{-\frac{1}{x}}} + \frac{1}{1 + e^{\frac{1}{x}}} = \frac{a}{a + 1} + \frac{1}{a + 1} = 1
\]
Thus, the integrand simplifies to \(\cos x\), so:
\[
2I = \int_{-1}^1 \cos x\, dx
\]

### Step 3: Evaluate the simplified integral
The integral of \(\cos x\) is \(\sin x\). Evaluating from \(-1\) to \(1\):
\[
\int_{-1}^1 \cos x\, dx = \sin(1) - \sin(-1) = \sin(1) + \sin(1) = 2\sin(1)
\]
Thus, \(2I = 2\sin(1)\), so \(I = \sin(1)\).

### Numerical Approximation
The numerical value of \(\sin(1)\) (where \(1\) is in radians) is approximately \(0.8414709848\) when rounded to 10 decimal places.

{"answer": "\(\sin(1)\)", "numerical_answer": "0.8414709848"}