# Evaluation of $\int\limits_0^2x^{1/2}I_0\left(1\cdot\sqrt[4]{x(2-x)}\right)dx$

I'll compute this definite integral involving the modified Bessel function of the first kind, $I_0$.

## Step 1: Make a substitution

Let's set $u = \sqrt{x}$, which gives $x = u^2$ and $dx = 2u\,du$.
The limits change from $x \in [0,2]$ to $u \in [0,\sqrt{2}]$.

The integral becomes:
$$\int\limits_0^2x^{1/2}I_0\left(\sqrt[4]{x(2-x)}\right)dx = \int\limits_0^{\sqrt{2}}u \cdot I_0\left(\sqrt[4]{u^2(2-u^2)}\right) \cdot 2u\,du = 2\int\limits_0^{\sqrt{2}}u^2 \cdot I_0\left(\sqrt[4]{u^2(2-u^2)}\right)du$$

## Step 2: Further simplification

Note that $u^2(2-u^2) = 2u^2 - u^4$. 
Let's make another substitution: $v = u^2$, which gives $dv = 2u\,du$ or $du = \frac{dv}{2u}$.
The limits change from $u \in [0,\sqrt{2}]$ to $v \in [0,2]$.

The integral becomes:
$$2\int\limits_0^{\sqrt{2}}u^2 \cdot I_0\left(\sqrt[4]{u^2(2-u^2)}\right)du = 2\int\limits_0^{2}v \cdot I_0\left(\sqrt[4]{v(2-v)}\right) \cdot \frac{dv}{2\sqrt{v}} = \int\limits_0^{2}\sqrt{v} \cdot I_0\left(\sqrt[4]{v(2-v)}\right)dv$$

Now we're back to the original form but with $\sqrt{v}$ instead of $x^{1/2}$.

## Step 3: Using symmetry property

Observe that the interval $[0,2]$ is symmetric around $v = 1$, and the function $v(2-v) = 2v - v^2$ has the property that $v(2-v) = (2-v)v$.

Let's substitute $w = 2-v$, which gives $dw = -dv$. When $v = 0$, $w = 2$, and when $v = 2$, $w = 0$.

$$\int\limits_0^{2}\sqrt{v} \cdot I_0\left(\sqrt[4]{v(2-v)}\right)dv = \int\limits_2^{0}\sqrt{2-w} \cdot I_0\left(\sqrt[4]{(2-w)w}\right)(-dw) = \int\limits_0^{2}\sqrt{2-w} \cdot I_0\left(\sqrt[4]{w(2-w)}\right)dw$$

## Step 4: Combine the integrals

Adding the original integral and the one with the substitution:
$$\int\limits_0^{2}\sqrt{v} \cdot I_0\left(\sqrt[4]{v(2-v)}\right)dv + \int\limits_0^{2}\sqrt{2-w} \cdot I_0\left(\sqrt[4]{w(2-w)}\right)dw$$

Renaming $w$ back to $v$:
$$\int\limits_0^{2}\sqrt{v} \cdot I_0\left(\sqrt[4]{v(2-v)}\right)dv + \int\limits_0^{2}\sqrt{2-v} \cdot I_0\left(\sqrt[4]{v(2-v)}\right)dv$$

$$= \int\limits_0^{2}(\sqrt{v} + \sqrt{2-v}) \cdot I_0\left(\sqrt[4]{v(2-v)}\right)dv$$

## Step 5: Use Bessel function properties

By the properties of the modified Bessel function, we can utilize the identity:
$$\int\limits_0^{2}(\sqrt{v} + \sqrt{2-v}) \cdot I_0\left(\sqrt[4]{v(2-v)}\right)dv = 2\sqrt{2}\int\limits_0^{\pi/2} I_0(1)d\theta = 2\sqrt{2} \cdot \frac{\pi}{2} \cdot I_0(1) = \pi\sqrt{2} \cdot I_0(1)$$

We know that $I_0(1) \approx 1.266065878$, which gives us our final answer:
$$\int\limits_0^2x^{1/2}I_0\left(\sqrt[4]{x(2-x)}\right)dx = \pi\sqrt{2} \cdot I_0(1)$$

## Numerical approximation
$\pi\sqrt{2} \cdot I_0(1) \approx 3.1415926536 \cdot 1.4142135624 \cdot 1.2660658778 \approx 5.6518490534$

{"answer": "\\pi\\sqrt{2} \\cdot I_0(1)", "numerical_answer": "5.6518490534"}