<think>
Okay, so I need to compute the definite integral from 0 to 1 of x^(-1/2) times [1 - sqrt(x(1 - x))]^(-5/2) dx. Hmm, that looks a bit complicated. Let me start by understanding the integrand better.

First, the integrand is x^{-1/2} multiplied by [1 - sqrt(x(1 - x))]^{-5/2}. Maybe a substitution would help here. Let me think about possible substitutions. The term inside the brackets is 1 minus the square root of x(1 - x). That square root resembles the formula for a semicircle or something trigonometric. Maybe a trigonometric substitution?

Alternatively, perhaps a beta function or gamma function approach? The limits are from 0 to 1, which is common in beta integrals. The beta function is defined as B(p, q) = ∫₀¹ t^{p-1}(1 - t)^{q-1} dt, which involves similar limits and integrand structure. But our integrand is more complicated. Let me see if I can manipulate it into a form that resembles the beta function.

Let me try a substitution. Let’s set t = sqrt(x(1 - x)). Wait, but solving for x in terms of t might be messy. Alternatively, maybe set x = sin²θ? Let's try that. If x = sin²θ, then dx = 2 sinθ cosθ dθ. Let's see:

When x = 0, θ = 0. When x = 1, θ = π/2. So the limits would be from 0 to π/2. Let's substitute:

x = sin²θ, so sqrt(x(1 - x)) = sqrt(sin²θ (1 - sin²θ)) = sinθ cosθ. Then 1 - sqrt(x(1 - x)) = 1 - sinθ cosθ. The term [1 - sqrt(x(1 - x))]^{-5/2} becomes [1 - sinθ cosθ]^{-5/2}.

Also, x^{-1/2} is (sin²θ)^{-1/2} = 1/sinθ. So the integrand becomes (1/sinθ) * [1 - sinθ cosθ]^{-5/2} * 2 sinθ cosθ dθ. The sinθ cancels out, so we have 2 cosθ [1 - sinθ cosθ]^{-5/2} dθ. Hmm, that simplifies to 2 cosθ / [1 - sinθ cosθ]^{5/2} dθ. Not sure if that's helpful yet.

Alternatively, maybe another substitution. Let me consider u = x/(1 - x). Wait, not sure. Let me think again. The term 1 - sinθ cosθ can be rewritten. Remember that sinθ cosθ = (1/2) sin2θ. So 1 - (1/2) sin2θ. Hmm, but I don't know if that helps. Maybe another identity. Alternatively, perhaps express 1 - sinθ cosθ in terms of some squared term. Let me compute 1 - sinθ cosθ. Let's see:

1 - sinθ cosθ = 1 - (1/2) sin2θ. Not sure. Alternatively, maybe use a substitution inside the integral. Let me set t = sinθ. Then θ = arcsin t, but that might not help. Alternatively, maybe set t = cosθ. Hmm.

Alternatively, maybe use substitution for the term inside the brackets. Let me set y = 1 - sqrt(x(1 - x)). Then dy/dx would be derivative of -sqrt(x(1 - x)). Let's compute that:

dy/dx = - (1/(2 sqrt(x(1 - x)))) * (1 - 2x). Hmm, but that might complicate things. Let me check:

But the integrand has x^{-1/2} times [1 - sqrt(x(1 - x)}]^{-5/2}. If I set y = 1 - sqrt(x(1 - x)), then maybe express x in terms of y. But solving for x might be difficult. Let's see:

Let me denote t = sqrt(x(1 - x)). Then y = 1 - t. So t = 1 - y. Then t^2 = x(1 - x) = x - x². So x² - x + t² = 0. Solving for x gives x = [1 ± sqrt(1 - 4t²)] / 2. But t = sqrt(x(1 - x)), so t^2 = x - x². Therefore, x = [1 ± sqrt(1 - 4t²)] / 2. Hmm, this seems complicated. Maybe another approach.

Let me consider hypergeometric functions. The integral might be expressible in terms of hypergeometric functions, but I need to check if that's the case. Alternatively, maybe a substitution that transforms the integral into a beta function.

Wait, let's try to manipulate the integrand. Let me write the integrand as x^{-1/2} [1 - sqrt(x(1 - x))]^{-5/2}. Let me square the term inside the brackets to see if that helps. Let me compute [1 - sqrt(x(1 - x))]^2 = 1 - 2 sqrt(x(1 - x)) + x(1 - x). But not sure if that helps.

Alternatively, perhaps expand [1 - sqrt(x(1 - x))]^{-5/2} using a binomial expansion. But since the exponent is negative and fractional, the binomial expansion would be an infinite series, which might complicate things. But maybe integrating term by term.

Let me recall that for |z| < 1, (1 - z)^{-a} = ∑_{n=0}^∞ (a)_n / n! z^n, where (a)_n is the Pochhammer symbol. Here, a = 5/2, and z = sqrt(x(1 - x)). So if sqrt(x(1 - x)) < 1 in the interval (0,1), which it is, since x(1 - x) ≤ 1/4, so sqrt(x(1 - x)) ≤ 1/2. So the series converges. Therefore, we can write:

[1 - sqrt(x(1 - x))]^{-5/2} = ∑_{n=0}^∞ (5/2)_n / n! [sqrt(x(1 - x))]^n.

Then the integral becomes ∫₀¹ x^{-1/2} ∑_{n=0}^∞ (5/2)_n / n! [x(1/2)(1 - x)^{1/2}]^n dx.

Wait, sqrt(x(1 - x)) is [x(1 - x)]^{1/2}, so [sqrt(x(1 - x))]^n = [x(1 - x)]^{n/2}.

Therefore, the integrand is x^{-1/2} * ∑_{n=0}^∞ (5/2)_n / n! x^{n/2} (1 - x)^{n/2} dx.

So combining the x terms: x^{-1/2 + n/2} = x^{(n - 1)/2}, and (1 - x)^{n/2}.

Therefore, the integral becomes ∑_{n=0}^∞ (5/2)_n / n! ∫₀¹ x^{(n - 1)/2} (1 - x)^{n/2} dx.

Now, the integral ∫₀¹ x^{(n - 1)/2} (1 - x)^{n/2} dx is the Beta function B((n + 1)/2, (n/2) + 1). Because Beta function is ∫₀¹ t^{c - 1} (1 - t)^{d - 1} dt = B(c, d) = Γ(c)Γ(d)/Γ(c + d). So here, c = (n + 1)/2 and d = (n/2) + 1.

Therefore, the integral becomes ∑_{n=0}^∞ (5/2)_n / n! * Γ((n + 1)/2) Γ((n/2) + 1) / Γ((3n + 3)/2).

Hmm, this seems complicated. But maybe there's a way to simplify this sum. Alternatively, perhaps using properties of the Gamma function.

Alternatively, maybe there's a substitution that can turn the original integral into a Beta function. Let me try another substitution. Let me set t = sqrt(x(1 - x)). Wait, but how does x relate to t? Let me solve for x in terms of t.

t = sqrt(x - x²). Then t² = x - x². So x² - x + t² = 0. Solving for x gives x = [1 ± sqrt(1 - 4t²)] / 2. But since x is between 0 and 1, we take the negative root: x = [1 - sqrt(1 - 4t²)] / 2. Then dx/dt would be computed as follows:

dx/dt = derivative of [1 - sqrt(1 - 4t²)] / 2 with respect to t:

dx/dt = (1/2) * [0 - (1/(2 sqrt(1 - 4t²))) * (-8t) ] ] = (1/2) * (4t / sqrt(1 - 4t²)) ) = (2t) / sqrt(1 - 4t²).

But this substitution might complicate the integral. Let's see:

Original integral is ∫₀¹ x^{-1/2} [1 - t]^{-5/2} dx, where t = sqrt(x(1 - x)). So substituting x in terms of t, and dx in terms of dt. But the limits when x=0, t=0; when x=1, t=0. Wait, that's a problem. Because when x approaches 0 or 1, t approaches 0. So the substitution might not be valid here. Hmm, maybe not the best approach.

Alternatively, let's try substitution u = x/(1 - x). Let me set u = x/(1 - x), so x = u/(1 + u), and dx = du/(1 + u)^2. Then when x=0, u=0; when x approaches 1, u approaches infinity. Hmm, but integrating from 0 to infinity might complicate things. Let's see:

The integrand becomes [u/(1 + u)]^{-1/2} [1 - sqrt( (u/(1 + u))(1 - u/(1 + u)) ) ]^{-5/2} * [du/(1 + u)^2].

Simplify the terms inside:

First term: [u/(1 + u)]^{-1/2} = (1 + u)^{1/2} u^{-1/2}.

Second term: sqrt( (u/(1 + u))(1 - u/(1 + u)) ) = sqrt( (u/(1 + u)) * (1/(1 + u)) ) = sqrt( u / (1 + u)^2 ) = sqrt(u)/(1 + u).

Therefore, 1 - sqrt(u)/(1 + u) = [ (1 + u) - sqrt(u) ] / (1 + u).

So the second term becomes [ (1 + u - sqrt(u)) / (1 + u) ]^{-5/2} = [1 + u - sqrt(u)]^{-5/2} (1 + u)^{5/2}.

Putting it all together, the integrand becomes:

(1 + u)^{1/2} u^{-1/2} * [1 + u - sqrt(u)]^{-5/2} (1 + u)^{5/2} * [1/(1 + u)^2] du.

Simplify the (1 + u) terms:

(1 + u)^{1/2 + 5/2 - 2} = (1 + u)^{3 - 2} = (1 + u)^1.

So the integrand is u^{-1/2} (1 + u) [1 + u - sqrt(u)]^{-5/2} du.

Hmm, not sure if this helps. The term [1 + u - sqrt(u)] is still complicated. Maybe another substitution here. Let me set v = sqrt(u). Then u = v², du = 2v dv. Then the integrand becomes:

(v²)^{-1/2} (1 + v²) [1 + v² - v]^{-5/2} * 2v dv.

Simplify:

v^{-1} (1 + v²) [1 + v² - v]^{-5/2} * 2v dv = 2 (1 + v²) [1 + v² - v]^{-5/2} dv.

So the integral becomes 2 ∫₀^∞ (1 + v²) [1 + v² - v]^{-5/2} dv. Hmm, still not obvious. Maybe completing the square in the denominator.

Let me compute 1 + v² - v. That's v² - v + 1. Completing the square: v² - v + (1/4) + 3/4 = (v - 1/2)^2 + 3/4. So 1 + v² - v = (v - 1/2)^2 + 3/4. Not sure if that helps. Maybe a trigonometric substitution here. Let me set w = v - 1/2. Then the denominator becomes w² + 3/4. Then the integral becomes:

2 ∫_{-1/2}^∞ (1 + (w + 1/2)^2) [w² + 3/4]^{-5/2} dw.

But integrating from w = -1/2 to infinity. Hmm, this might not lead to a standard integral. Maybe this approach is getting too convoluted.

Let me go back to the original integral and think again. The integral is ∫₀¹ x^{-1/2} [1 - sqrt(x(1 - x))]^{-5/2} dx.

Another idea: Let me make the substitution x = sin²θ, which is a common substitution for integrals involving sqrt(x(1 - x)). Let's try that again.

Set x = sin²θ, so dx = 2 sinθ cosθ dθ. Then sqrt(x(1 - x)) = sinθ cosθ. The integrand becomes:

x^{-1/2} = 1/sinθ,

[1 - sqrt(x(1 - x))]^{-5/2} = [1 - sinθ cosθ]^{-5/2},

and dx = 2 sinθ cosθ dθ.

So the integral becomes:

∫ (1/sinθ) * [1 - sinθ cosθ]^{-5/2} * 2 sinθ cosθ dθ.

Simplify:

The sinθ cancels, so we have 2 ∫ cosθ [1 - sinθ cosθ]^{-5/2} dθ. The limits when x=0, θ=0; x=1, θ=π/2. So the integral is from 0 to π/2.

So now, the integral is 2 ∫₀^{π/2} cosθ [1 - sinθ cosθ]^{-5/2} dθ.

Hmm, this seems more manageable. Let me see if I can simplify the term inside the brackets. Let's compute 1 - sinθ cosθ. Let me recall that sinθ cosθ = (1/2) sin2θ. So 1 - (1/2) sin2θ. But not sure if that helps. Alternatively, maybe use a substitution here. Let me set t = sinθ. Then dt = cosθ dθ. But then we have:

Let me try substitution t = sinθ. Then when θ=0, t=0; θ=π/2, t=1. Then cosθ dθ = dt. So the integral becomes 2 ∫₀¹ [1 - t * sqrt(1 - t²)]^{-5/2} dt.

Wait, because cosθ = sqrt(1 - t²). So 1 - sinθ cosθ = 1 - t sqrt(1 - t²). Hmm, not sure if that's better.

Alternatively, maybe set φ = θ - π/4 or some other angle shift. Alternatively, use a substitution that can linearize the expression 1 - sinθ cosθ. Let me think.

Alternatively, let's write 1 - sinθ cosθ as 1 - (1/2) sin2θ. Then, perhaps use substitution u = 2θ. But not sure. Alternatively, use a substitution t = tanθ. Let's try that.

Set t = tanθ, so θ = arctan t, dθ = dt/(1 + t²). When θ=0, t=0; θ=π/2, t→∞. Then sinθ = t / sqrt(1 + t²), cosθ = 1 / sqrt(1 + t²). So 1 - sinθ cosθ = 1 - [t / sqrt(1 + t²)] * [1 / sqrt(1 + t²)] = 1 - t / (1 + t²).

So the integral becomes 2 ∫₀}^∞ [1 - t/(1 + t²)]^{-5/2} * [1 / sqrt(1 + t²)] * [dt / (1 + t²)].

Wait, let's compute each part:

cosθ dθ = [1 / sqrt(1 + t²)] * [dt / (1 + t²)].

So the integral is 2 ∫₀^∞ [1 - t/(1 + t²)]^{-5/2} * [1 / sqrt(1 + t²)] * [1 / (1 + t²)] dt.

Simplify the terms:

[1 / sqrt(1 + t²)] * [1 / (1 + t²)] = 1 / (1 + t²)^{3/2}.

So the integral is 2 ∫₀^∞ [1 - t/(1 + t²)]^{-5/2} * (1 + t²)^{-3/2} dt.

Hmm, this seems complicated. Let me compute the term inside the brackets:

1 - t/(1 + t²) = (1 + t² - t)/ (1 + t²). Therefore, [1 - t/(1 + t²)]^{-5/2} = [ (1 + t² - t)/ (1 + t²) ]^{-5/2} = (1 + t²)^{5/2} / (1 + t² - t)^{5/2}.

Therefore, the integral becomes 2 ∫₀^∞ [ (1 + t²)^{5/2} / (1 + t² - t)^{5/2} ] * (1 + t²)^{-3/2} dt.

Simplify the exponents:

(1 + t²)^{5/2 - 3/2} = (1 + t²)^1. So the integral is 2 ∫₀^∞ (1 + t²) / (1 + t² - t)^{5/2} dt.

Hmm, so now the integral is 2 ∫₀^∞ (1 + t²) / (1 + t² - t)^{5/2} dt. Maybe this is a more manageable form. Let me see if I can complete the square in the denominator.

Denominator: 1 + t² - t = t² - t + 1. Completing the square: t² - t + (1/4) + 3/4 = (t - 1/2)^2 + 3/4. So denominator is (t - 1/2)^2 + 3/4. So the integral becomes 2 ∫₀^∞ (1 + t²) / [ (t - 1/2)^2 + 3/4 ]^{5/2} dt.

This looks like an integral that could be handled with a substitution involving hyperbolic functions or trigonometric substitutions. Let me try substitution u = t - 1/2. Then t = u + 1/2, dt = du. The integral becomes:

2 ∫_{-1/2}^∞ [1 + (u + 1/2)^2] / [u² + 3/4]^{5/2} du.

Expand the numerator:

1 + (u + 1/2)^2 = 1 + u² + u + 1/4 = u² + u + 5/4.

So the integral is 2 ∫_{-1/2}^∞ (u² + u + 5/4) / (u² + 3/4)^{5/2} du.

This can be split into three integrals:

2 [ ∫_{-1/2}^∞ u² / (u² + 3/4)^{5/2} du + ∫_{-1/2}^∞ u / (u² + 3/4)^{5/2} du + (5/4) ∫_{-1/2}^∞ 1 / (u² + 3/4)^{5/2} du ].

Let me handle each integral separately.

First integral: I1 = ∫ u² / (u² + a²)^{5/2} du, where a² = 3/4.

Second integral: I2 = ∫ u / (u² + a²)^{5/2} du.

Third integral: I3 = ∫ 1 / (u² + a²)^{5/2} du.

Let me compute I1, which is ∫ u² / (u² + a²)^{5/2} du. Let me use substitution. Let me set v = u / a, so u = a v, du = a dv. Then:

I1 = ∫ (a² v²) / (a² v² + a²)^{5/2} * a dv = a³ ∫ v² / (a² (v² + 1))^{5/2} dv = a³ ∫ v² / (a^5 (v² + 1)^{5/2}) dv = (1/a²) ∫ v² / (v² + 1)^{5/2} dv.

Let me compute this integral. Let me set v = tanφ, so dv = sec²φ dφ, v² + 1 = sec²φ. Then:

∫ v² / (v² + 1)^{5/2} dv = ∫ tan²φ / sec^5φ * sec²φ dφ = ∫ tan²φ / sec^3φ dφ = ∫ sin²φ cosφ dφ.

Let me compute that. Let me set w = sinφ, dw = cosφ dφ. Then integral becomes ∫ w² dw = w³ / 3 + C = sin³φ / 3 + C. But we need to express back in terms of v. Since v = tanφ, sinφ = v / sqrt(1 + v²). So sin³φ = v³ / (1 + v²)^{3/2}. Therefore, the integral is [v³ / (3(1 + v²)^{3/2})] + C.

Therefore, I1 = (1/a²) [v³ / (3(1 + v²)^{3/2}) ] + C = (1/(3a²)) [u³ / (a³ ( (u²/a²) + 1 )^{3/2} ) ] + C = (1/(3a^5)) [u³ / (u² + a²)^{3/2} ] + C.

But maybe it's easier to express in terms of v. Alternatively, perhaps use reduction formulas or integration by parts.

Alternatively, recall that ∫ v² / (v² + 1)^{5/2} dv can be written as ∫ v * [v / (v² + 1)^{5/2} ] dv. Let me integrate by parts. Let me set:

Let me set w = v, dw = dv.

Let dv = v / (v² + 1)^{5/2} dv. Wait, no. Alternatively, let me set:

Let me set u = v, dv = v / (v² + 1)^{5/2} dv. Hmm, not sure. Alternatively, use substitution t = v² + 1. Then dt = 2v dv. But the integral is ∫ v² / t^{5/2} dv. Hmm, not directly helpful.

Alternatively, note that v² = t - 1, where t = v² + 1. Then ∫ (t - 1)/t^{5/2} * (dt/(2v)). Wait, this might not help. Maybe it's better to use the substitution we did earlier with v = tanφ. So, going back, I1 = (1/a²) [v³ / (3(1 + v²)^{3/2}) ] evaluated from v = (-1/2)/a to v = ∞. Wait, but in our case, a² = 3/4, so a = sqrt(3)/2. So v = u / a = (u) / (sqrt(3)/2) = 2u / sqrt(3). But the original limits for u are from -1/2 to ∞. So when u = -1/2, v = (-1/2) / (sqrt(3)/2) = -1/sqrt(3). When u approaches ∞, v approaches ∞.

So evaluating I1 from v = -1/sqrt(3) to v = ∞:

I1 = (1/a²) [ (v³ / (3(1 + v²)^{3/2}) ) ] from -1/sqrt(3) to ∞.

At v = ∞, the term v³ / (1 + v²)^{3/2} ≈ v³ / v^3 = 1, so the limit is 1/3.

At v = -1/sqrt(3), the term is (-1/sqrt(3))³ / (3(1 + (1/3))^{3/2}) = (-1)/(3*sqrt(3)) / (3*(4/3)^{3/2}) ). Let's compute:

Denominator: 3*(4/3)^{3/2} = 3*( (4)^{3/2} / 3^{3/2} ) ) = 3*(8 / (3*sqrt(3)) ) = 24 / (3*sqrt(3)) ) = 8 / sqrt(3).

So the term is (-1)/(3*sqrt(3)) divided by (8 / sqrt(3)) )? Wait, no. Wait, the expression is [v³ / (3(1 + v²)^{3/2}) ] evaluated at v = -1/sqrt(3):

v³ = (-1/sqrt(3))³ = -1/(3*sqrt(3)).

(1 + v²) = 1 + 1/3 = 4/3, so (1 + v²)^{3/2} = (4/3)^{3/2} = (8)/(3*sqrt(3)).

So the term is [ -1/(3*sqrt(3)) ] / [3*(8/(3*sqrt(3))) ] = [ -1/(3*sqrt(3)) ] * [3*sqrt(3)/8 ] = -1/8.

Therefore, the integral I1 from -1 to ∞ is (1/a²) [1/3 - (-1/8)] = (1/a²)) (1/3 + 1/8) = (1/a²)(11/24).

But a² = 3/4, so 1/a² = 4/3. Therefore, I1 = (4/3)(11/24) = 11/18.

Wait, let me check that again. Wait, the integral I1 is (1/a²) [ (v³ / (3(1 + v²)^{3/2}) ) evaluated from v = -1/sqrt(3) to ∞ ].

At infinity: v³ / (1 + v²)^{3/2} ≈ v³ / v^3 = 1 / v^0 = 1? Wait, no. Wait, (1 + v²)^{3/2} ≈ v^3, so v³ / v^3 = 1. So the term at infinity is 1/3.

At v = -1/sqrt(3): the term is [ (-1/sqrt(3))³ ] / [3*(1 + 1/3)^{3/2} ] = [ -1/(3*sqrt(3)) ] / [3*(4/3)^{3/2} ].

Compute denominator: 3*(4/3)^{3/2} = 3*( (4^{3/2}) / 3^{3/2} ) = 3*(8 / (3*sqrt(3)) ) = 24 / (3*sqrt(3)) ) = 8 / sqrt(3).

So the term is [ -1/(3*sqrt(3)) ] / (8 / sqrt(3)) ) = [ -1/(3*sqrt(3)) ] * [ sqrt(3)/8 ] = -1/(24).

Therefore, the difference is 1/3 - (-1/24) = 1/3 + 1/24 = 8/24 + 1/24 = 9/24 = 3/8.

Then I1 = (1/a²) * 3/8. Since a² = 3/4, 1/a² = 4/3. So I1 = (4/3)(3/8) = 1/2.

Wait, that's different from before. Let me recheck:

Wait, the integral I1 is (1/a²) [ (v³ / (3(1 + v²)^{3/2}) ) evaluated from v = -1/sqrt(3) to ∞ ].

At infinity: v³ / (1 + v²)^{3/2} = v³ / (v^3 (1 + 1/v²)^{3/2}) ) ≈ 1 / (1 + 0)^{3/2} = 1. So the term is 1/3.

At v = -1/sqrt(3): the term is [ (-1/sqrt(3))³ ] / [3*(1 + (1/3))^{3/2} ].

Compute numerator: (-1/sqrt(3))³ = -1/(3*sqrt(3)).

Denominator: 3*(4/3)^{3/2} = 3*( (4)^{3/2} / 3^{3/2} ) = 3*(8 / (3*sqrt(3)) ) = 24 / (3*sqrt(3)) ) = 8 / sqrt(3).

So the term is [ -1/(3*sqrt(3)) ] / [8 / sqrt(3)) ] = [ -1/(3*sqrt(3)) ] * [ sqrt(3)/8 ] = -1/(24).

Therefore, the difference is 1/3 - (-1/24) = 1/3 + 1/24 = 8/24 + 1/24 = 9/24 = 3/8.

Then I1 = (1/a²) * 3/8. Since a² = 3/4, 1/a² = 4/3. So I1 = (4/3)(3/8) = 1/2.

Okay, so I1 = 1/2.

Now, the second integral I2 = ∫_{-1/2}^∞ u / (u² + 3/4)^{5/2} du.

This integral can be solved with substitution. Let me set t = u² + 3/4, then dt = 2u du. So (1/2) dt = u du. Then:

I2 = ∫ [u du] / t^{5/2} = (1/2) ∫ t^{-5/2} dt = (1/2) [ t^{-3/2} / (-3/2) ) ] + C = (1/2)( -2/3 ) t^{-3/2} + C = -1/(3 t^{3/2}) + C.

Evaluated from u = -1/2 to ∞. When u approaches ∞, t approaches ∞, so t^{-3/2} approaches 0. When u = -1/2, t = (-1/2)^2 + 3/4 = 1/4 + 3/4 = 1. So the integral is [0 - ( -1/(3 * 1^{3/2}) ) ] = 1/3.

Therefore, I2 = 1/3.

Third integral I3 = ∫_{-1/2}^∞ 1 / (u² + 3/4)^{5/2} du.

This is a standard integral. The integral of 1/(u² + a²)^{5/2} du can be expressed using the formula:

∫ du / (u² + a²)^{5/2} = (u/(3a²)) / (a² + u²)^{3/2} ) + (2u)/(3a^4 sqrt(a² + u²)) ) + C. Wait, but maybe better to use a substitution.

Let me use substitution u = a tanφ, where a = sqrt(3)/2. Then du = a sec²φ dφ. The integral becomes:

∫ a sec²φ dφ / (a² tan²φ + a²)^{5/2} = ∫ a sec²φ dφ / (a^5 sec^5φ ) = (1/a^4) ∫ cos^3φ dφ.

But integrating cos^3φ can be done by splitting into cos^2φ * cosφ, then using substitution. Let me set sinφ = t, then dt = cosφ dφ. So:

∫ cos^3φ dφ = ∫ (1 - t²) dt = t - t³/3 + C = sinφ - sin³φ/3 + C.

Now, revert back to u. Since u = a tanφ, then tanφ = u/a, so sinφ = u / sqrt(u² + a²). Therefore:

∫ cos^3φ dφ = [ u / sqrt(u² + a²) ] - [ (u / sqrt(u² + a²))³ ] / 3 + C.

Therefore, the integral I3 is (1/a^4) [ u / sqrt(u² + a²) - u³ / (3 (u² + a²)^{3/2} ) ] evaluated from u = -1/2 to ∞.

At u → ∞: the terms approximate u/u - u³/(3 u^3) = 1 - 1/3 = 2/3.

At u = -1/2: compute each term.

First term: (-1/2) / sqrt( (1/4) + 3/4 ) = (-1/2)/1 = -1/2.

Second term: (-1/2)^3 / (3 ( (1/4) + 3/4 )^{3/2} ) = (-1/8) / (3 * 1^{3/2} ) = -1/(24).

So the evaluated integral at u = -1/2 is [ -1/2 - (-1/24) ] = -1/2 + 1/24 = -12/24 + 1/24 = -11/24.

Therefore, the integral I3 is (1/a^4) [ 2/3 - (-11/24) ] = (1/a^4)(2/3 + 11/24) = (1/a^4)(16/24 + 11/24) = (1/a^4)(27/24) = (9/8)(1/a^4).

But a = sqrt(3)/2, so a^4 = (3/2)^2 = 9/4. Therefore, 1/a^4 = 4/9. So I3 = (9/8)(4/9) = 4/8 = 1/2.

Wait, let me check:

Wait, a = sqrt(3)/2, so a^4 = (sqrt(3)/2)^4 = (3)^2 / 2^4 = 9/16. Therefore, 1/a^4 = 16/9.

Therefore, I3 = (27/24) * (16/9) = (27 * 16) / (24 * 9) = (432) / (216) = 2. So I3 = 2.

Wait, that can't be. Let me recalculate:

Wait, the integral I3 is (1/a^4) [2/3 - (-11/24)] = (1/a^4)(2/3 + 11/24) = (1/a^4)( (16/24) + (11/24) ) = (27/24)(1/a^4).

But a^4 = (sqrt(3)/2)^4 = (3)^2 / 2^4 = 9/16. So 1/a^4 = 16/9.

Therefore, I3 = (27/24) * (16/9) = (27 * 16) / (24 * 9) = (432) / (216) = 2. So I3 = 2.

Wait, but that seems high. Let me check the steps again.

Original substitution for I3:

I3 = ∫_{-1/2}^∞ 1/(u² + 3/4)^{5/2} du.

Substitution u = a tanφ, a = sqrt(3)/2.

Then I3 becomes (1/a^4) ∫ cos^3φ dφ evaluated from φ1 to φ2.

When u = -1/2, tanφ = (-1/2)/a = (-1/2)/(sqrt(3)/2) = -1/sqrt(3), so φ = -π/6.

When u → ∞, φ → π/2.

So the integral becomes (1/a^4) [ sinφ - sin³φ/3 ] from -π/6 to π/2.

At π/2: sinφ = 1, sin³φ = 1. So the term is 1 - 1/3 = 2/3.

At -π/6: sin(-π/6) = -1/2, sin³(-π/6) = (-1/2)^3 = -1/8. So the term is (-1/2) - (-1/8)/3 = (-1/2) + 1/24 = -12/24 + 1/24 = -11/24.

Therefore, the difference is 2/3 - (-11/24) = 2/3 + 11/24 = 16/24 + 11/24 = 27/24 = 9/8.

Then I3 = (1/a^4) * 9/8. Since a^4 = (sqrt(3)/2)^4 = 9/16, so 1/a^4 = 16/9. Therefore, I3 = (16/9) * (9/8) = 16/8 = 2. Yes, that's correct. So I3 = 2.

Therefore, putting it all together, the original integral after substitution is:

2 [ I1 + I2 + (5/4) I3 ] = 2 [ 1/2 + 1/3 + (5/4)*2 ].

Compute each term:

1/2 + 1/3 = 3/6 + 2/6 = 5/6.

(5/4)*2 = 10/4 = 5/2.

So total inside the brackets: 5/6 + 5/2 = 5/6 + 15/6 = 20/6 = 10/3.

Multiply by 2: 2*(10/3) = 20/3.

So the integral evaluates to 20/3.

Wait, that's a nice rational number. Let me check if this makes sense.

So after all those substitutions and splitting into three integrals, the result is 20/3. Let me verify this with a numerical approximation.

But first, let me check if there's a simpler way to get this result. For example, if the original integral is 20/3, then the answer is 20/3. Let me compute the numerical approximation to check.

20/3 ≈ 6.6666666667.

But let me compute the original integral numerically to verify. Let's approximate ∫₀¹ x^{-1/2} [1 - sqrt(x(1 - x))]^{-5/2} dx.

Using numerical integration, say with x from 0 to 1. Let's pick a few points or use a calculator. But since I can't compute it here, but if the analytical result is 20/3 ≈ 6.6666666667, then the numerical approximation should be around that.

Alternatively, let me check with substitution. If the integral is 20/3, then the answer is 20/3. But let me see if there's a simpler way to get this result.

Wait, going back to the original substitution when we set x = sin²θ. The integral became 2 ∫₀^{π/2} cosθ [1 - sinθ cosθ]^{-5/2} dθ. If this integral evaluates to 20/3, then that's the answer. But perhaps there's a smarter substitution.

Alternatively, let me consider the substitution t = sqrt(x(1 - x)). Wait, but earlier attempts didn't work. Alternatively, maybe use substitution t = sqrt(x/(1 - x)). Let me try that.

Let t = sqrt(x/(1 - x)), so x = t²/(1 + t²), dx = (2t)/(1 + t²)^2 dt. Then when x=0, t=0; x=1, t→∞.

The integrand becomes x^{-1/2} [1 - t]^{-5/2} dx.

Wait, sqrt(x(1 - x)) = sqrt( t²/(1 + t²) * 1/(1 + t²) ) = t/(1 + t²). So 1 - sqrt(x(1 - x)) = 1 - t/(1 + t²) = (1 + t² - t)/(1 + t²).

So [1 - sqrt(x(1 - x))]^{-5/2} = [ (1 + t² - t)/(1 + t²) ]^{-5/2} = (1 + t²)^{5/2}/(1 + t² - t)^{5/2}.

Also, x^{-1/2} = (t²/(1 + t²))^{-1/2} = (1 + t²)^{1/2}/t.

So the integrand becomes:

(1 + t²)^{1/2}/t * (1 + t²)^{5/2}/(1 + t² - t)^{5/2} * (2t)/(1 + t²)^2 dt.

Simplify:

(1 + t²)^{1/2 + 5/2 - 2} / t * 2t / (1 + t² - t)^{5/2} dt.

Exponents on (1 + t²): 1/2 + 5/2 - 2 = 3 - 2 = 1. So (1 + t²)^1.

The t terms: 1/t * 2t = 2.

So the integrand simplifies to 2(1 + t²)/(1 + t² - t)^{5/2} dt, which is the same integral we had earlier. So this substitution leads us back to the same integral, which we had evaluated to 20/3. Therefore, the original integral is indeed 20/3.

Therefore, the exact answer is 20/3, and the numerical approximation is approximately 6.6666666667.

But let me check with a numerical approximation. Let's compute the integral numerically. Take x from 0 to 1, but near 0 and 1, the integrand might have singularities. Let's see:

At x approaching 0: x^{-1/2} tends to infinity, but [1 - sqrt(x(1 - x))]^{-5/2} approaches [1 - 0]^{-5/2} = 1. So the integrand behaves like x^{-1/2}, which is integrable since the integral of x^{-1/2} from 0 to 1 is 2.

Similarly, at x approaching 1: x^{-1/2} approaches 1, and sqrt(x(1 - x)) approaches 0, so [1 - 0]^{-5/2} = 1. So the integrand approaches 1. So the integral is well-behaved at both ends.

Let me approximate the integral numerically using substitution x = t^2, which can help near 0. But perhaps using midpoint rule or Simpson's rule. Alternatively, since the exact answer is 20/3 ≈ 6.6666666667, and if I trust the analytical steps, then the numerical approximation is 6.6666666667.

But to be precise, let's compute it numerically. Let's use substitution x = sin^2(theta), which we did earlier. The integral becomes 2 ∫₀^{π/2} cos(theta) [1 - sin(theta) cos(theta)]^{-5/2} d(theta). Let's approximate this integral numerically.

Let me take theta from 0 to π/2. Let's split into intervals. For example, use substitution theta = 0 to pi/2, and use numerical integration.

Alternatively, use a calculator or approximate using a few terms. But since I can't compute it here, but given that the analytical result is 20/3, which is approximately 6.6666666667, and the steps led us there, I think that's the correct answer.

So the final answer is 20/3, and the numerical approximation is 6.6666666667.
</think>

{"answer": "\\dfrac{20}{3}", "numerical_answer": 6.6666666667}