Let's compute the definite integral step by step:

\[
\int_0^1 \left(e^{e^x} - e^{e^x - x}\right) dx
\]

### Step 1: Split the Integral
First, split the integral into two parts:

\[
\int_0^1 e^{e^x} dx - \int_0^1 e^{e^x - x} dx
\]

### Step 2: Simplify the Second Integral
For the second integral, let’s make a substitution to simplify it. Let \( u = e^x \), then \( du = e^x dx \) or \( dx = \frac{du}{u} \). When \( x = 0 \), \( u = 1 \), and when \( x = 1 \), \( u = e \).

The second integral becomes:

\[
\int_0^1 e^{e^x - x} dx = \int_{1}^{e} e^{u} \cdot e^{-\ln u} \cdot \frac{du}{u} = \int_{1}^{e} e^{u} \cdot \frac{1}{u} \cdot \frac{du}{u} = \int_{1}^{e} \frac{e^{u}}{u^2} du
\]

However, this substitution doesn't seem to simplify the integral. Let’s try another approach.

### Step 3: Combine the Integrals
Notice that the integrand can be rewritten as:

\[
e^{e^x} - e^{e^x - x} = e^{e^x} \left(1 - e^{-x}\right)
\]

But this doesn't immediately help. Instead, let’s consider the substitution \( v = e^x \), \( dv = e^x dx \), \( dx = \frac{dv}{v} \):

\[
\int_0^1 e^{e^x} dx = \int_{1}^{e} \frac{e^{v}}{v} dv
\]

\[
\int_0^1 e^{e^x - x} dx = \int_{1}^{e} \frac{e^{v}}{v^2} dv
\]

Now, the integral becomes:

\[
\int_{1}^{e} \frac{e^{v}}{v} dv - \int_{1}^{e} \frac{e^{v}}{v^2} dv
\]

### Step 4: Integrate by Parts
For the second integral, integrate by parts:

Let \( w = \frac{1}{v} \), \( dw = -\frac{1}{v^2} dv \), and \( dz = e^{v} dv \), \( z = e^{v} \).

Then:

\[
\int \frac{e^{v}}{v^2} dv = -\frac{e^{v}}{v} + \int \frac{e^{v}}{v} dv
\]

Thus, the second integral evaluates to:

\[
\int_{1}^{e} \frac{e^{v}}{v^2} dv = -\frac{e^{v}}{v} \Bigg|_{1}^{e} + \int_{1}^{e} \frac{e^{v}}{v} dv = -\frac{e^{e}}{e} + \frac{e^{1}}{1} + \int_{1}^{e} \frac{e^{v}}{v} dv = -e^{e-1} + e + \int_{1}^{e} \frac{e^{v}}{v} dv
\]

Now, substitute back into the original expression:

\[
\int_{1}^{e} \frac{e^{v}}{v} dv - \left(-e^{e-1} + e + \int_{1}^{e} \frac{e^{v}}{v} dv\right) = e^{e-1} - e
\]

### Step 5: Final Answer
The exact value of the integral is:

\[
e^{e - 1} - e
\]

### Step 6: Numerical Approximation
Now, compute the numerical approximation:

\[
e^{e - 1} - e \approx e^{1.7182818285} - e \approx 5.5749415226 - 2.7182818285 \approx 2.8566596941
\]

### Final Answer in JSON
```json
{"answer": "e^{e - 1} - e", "numerical_answer": "2.8566596941"}
```