To compute the definite integral 

\[
\int_0^1 (x-1)^2(x+1)^2(x^2+1)^2(x^4+1)^2 \, dx,
\]

we will follow these steps:

### Step 1: Simplify the Integrand

First, observe that the integrand can be simplified by recognizing patterns and using algebraic identities.

1. **Combine \((x-1)^2(x+1)^2\):**
   \[
   (x-1)^2(x+1)^2 = \left((x-1)(x+1)\right)^2 = (x^2 - 1)^2.
   \]
   
2. **Now, the integrand becomes:**
   \[
   (x^2 - 1)^2 (x^2 + 1)^2 (x^4 + 1)^2.
   \]
   
3. **Combine \((x^2 - 1)^2(x^2 + 1)^2\):**
   \[
   (x^2 - 1)^2(x^2 + 1)^2 = \left((x^2 - 1)(x^2 + 1)\right)^2 = (x^4 - 1)^2.
   \]
   
4. **Now, the integrand is:**
   \[
   (x^4 - 1)^2 (x^4 + 1)^2.
   \]
   
5. **Combine \((x^4 - 1)^2(x^4 + 1)^2\):**
   \[
   (x^4 - 1)^2(x^4 + 1)^2 = \left((x^4 - 1)(x^4 + 1)\right)^2 = (x^8 - 1)^2.
   \]
   
6. **Final simplified integrand:**
   \[
   (x^8 - 1)^2 = x^{16} - 2x^8 + 1.
   \]

### Step 2: Integrate the Simplified Expression

Now, integrate the simplified expression from 0 to 1:

\[
\int_0^1 (x^{16} - 2x^8 + 1) \, dx.
\]

Compute the integral term by term:

1. **Integrate \(x^{16}\):**
   \[
   \int x^{16} \, dx = \frac{x^{17}}{17}.
   \]
   
2. **Integrate \(-2x^8\):**
   \[
   \int -2x^8 \, dx = -\frac{2x^9}{9}.
   \]
   
3. **Integrate \(1\):**
   \[
   \int 1 \, dx = x.
   \]
   
4. **Combine the results and evaluate from 0 to 1:**
   \[
   \left. \frac{x^{17}}{17} - \frac{2x^9}{9} + x \right|_0^1 = \left(\frac{1}{17} - \frac{2}{9} + 1\right) - 0 = \frac{1}{17} - \frac{2}{9} + 1.
   \]
   
5. **Simplify the expression:**
   \[
   1 + \frac{1}{17} - \frac{2}{9} = \frac{153}{153} + \frac{9}{153} - \frac{34}{153} = \frac{153 + 9 - 34}{153} = \frac{128}{153}.
   \]

### Step 3: Numerical Approximation

Compute the numerical value of \(\frac{128}{153}\):

\[
\frac{128}{153} \approx 0.83660130719.
\]

### Final Answer

The exact answer is \(\frac{128}{153}\), and its numerical approximation is approximately 0.83660130719.

```json
{"answer": "\\frac{128}{153}", "numerical_answer": "0.8366013072"}
```