Let's solve the integral step by step:

\[
I = \int_1^{e^e} \frac{\log\left(x^{\log(x^x)}\right)}{x^2}\,dx
\]

### Step 1: Simplify the integrand

First, recall that \(\log(x^a) = a\log x\).

But inside, we have \(x^{\log(x^x)}\). Recall \(\log(a^b) = b \log a\):

\[
\log(x^{\log(x^x)}) = \log(x^x) \cdot \log x
\]

But \(\log(x^x) = x\log x\):

\[
\log(x^{\log(x^x)}) = (x\log x) \cdot \log x = x (\log x)^2
\]

Update the integral:

\[
I = \int_1^{e^e} \frac{x (\log x)^2}{x^2} dx = \int_1^{e^e} \frac{(\log x)^2}{x} dx
\]

### Step 2: Find the antiderivative

Recall:

\[
\int (\log x)^n \frac{dx}{x} = \frac{(\log x)^{n+1}}{n+1} + C
\]

For \(n=2\):

\[
\int (\log x)^2 \frac{dx}{x} = \frac{(\log x)^3}{3} + C
\]

### Step 3: Evaluate the definite integral

Apply limits \(1\) to \(e^e\):

\[
I = \left. \frac{(\log x)^3}{3} \right|_1^{e^e} = \frac{1}{3} \left( [\log(e^e)]^3 - [\log(1)]^3 \right)
\]

\[
\log(e^e) = e
\]
\[
\log(1) = 0
\]

Therefore,

\[
I = \frac{1}{3} (e^3 - 0) = \frac{e^3}{3}
\]

### Step 4: Numerical approximation

Using \(e \approx 2.7182818285\):

\[
e^3 \approx 2.7182818285^3 \approx 20.0855369232
\]
\[
I \approx \frac{20.0855369232}{3} \approx 6.6951789744
\]

### JSON Output

```json
{"answer": "\\frac{e^3}{3}", "numerical_answer": "6.6951789744"}
```