Let's solve the integral
\[
\int_0^1 \lfloor \log_{2023} x \rfloor \, dx
\]

**Step 1: Analyze the function \(\lfloor\log_{2023}x\rfloor\) on \([0,1]\)**

- For \(x=1\): \(\log_{2023}1 = 0\).
- As \(x\) goes from 1 down to 0, \(\log_{2023}x\) decreases from 0 to \(-\infty\).
- The value \(\lfloor\log_{2023}x\rfloor = n\) for \(x\) in the interval \([2023^{n}, 2023^{n+1})\), but since \(x \in [0,1]\), \(n\) is negative or zero.

For \(x\) between \(2023^{k}\) and \(2023^{k+1}\) where \(k \leq -1\), \(\lfloor\log_{2023}x\rfloor = k\).

Find which \(k\) are relevant for \(x\) in \([0,1]\):

- \(2023^{k} \leq x < 2023^{k+1}\)
- But since \(x \in [0,1]\), so \(k \leq 0\).
- \(2023^{k} \leq 1\) if \(k \leq 0\)
- The lowest value is as \(k \to -\infty\), \(2023^{k} \to 0\),
- The highest value \(k = 0 \Rightarrow x \in [1, 2023)\), but since our interval is up to 1, only \(x=1\) hits this.

So, partition:
- For \(k = -1, -2, -3, \ldots\):
    \(x \in [2023^{k}, 2023^{k+1})\), with \(2023^{k} \in (0,1)\), \(2023^{k+1} < 2023^{k} < 1\).
- The sum of all intervals \([2023^{k}, 2023^{k+1})\) for \(k = -1, -2, -3, \ldots\), union \(\{1\}\) as the endpoint.

But at \(x=1\), \(\log_{2023}1 = 0\), so \(\lfloor\log_{2023}1\rfloor = 0\), but the set \(\{1\}\) has measure zero, so it doesn't contribute to the integral.

**Step 2: Set up the sum over k**

\[
\int_0^1 \lfloor\log_{2023}x\rfloor dx = \sum_{k=-\infty}^{-1} \int_{2023^{k}}^{2023^{k+1}} k \, dx
= \sum_{k=-\infty}^{-1} k (2023^{k+1} - 2023^{k})
\]

**Step 3: Simplify the expression**

\(2023^{k+1} - 2023^{k} = 2023^{k}(2023 - 1) = 2023^{k} \cdot 2022\)

So,

\[
\int_0^1 \lfloor\log_{2023}x\rfloor dx = \sum_{k=-\infty}^{-1} k \cdot 2023^{k} \cdot 2022
= 2022 \sum_{k=-\infty}^{-1} k \cdot 2023^{k}
\]

Letâ€™s change the index: set \(n = -k\), so as \(k \to -\infty\), \(n \to +\infty\), and as \(k = -1\), \(n=1\):

\[
\sum_{k=-\infty}^{-1} k \cdot 2023^k = \sum_{n=1}^{\infty} (-n) \cdot 2023^{-n} = -\sum_{n=1}^\infty n \cdot 2023^{-n}
\]

Therefore,

\[
\int_0^1 \lfloor\log_{2023}x\rfloor dx = 2022 \left[ -\sum_{n=1}^{\infty} n \cdot 2023^{-n} \right ]
= -2022 \sum_{n=1}^\infty n \cdot 2023^{-n}
\]

**Step 4: Summing the series**

\(\sum_{n=1}^\infty n r^n = \frac{r}{(1 - r)^2}\) for \(|r| < 1\).

Here, \(r = \frac{1}{2023}\):

\[
\sum_{n=1}^{\infty} n \cdot 2023^{-n} = \frac{\frac{1}{2023}}{(1 - \frac{1}{2023})^2}
= \frac{1}{2023} \cdot \frac{1}{\left(\frac{2022}{2023}\right)^2}
= \frac{1}{2023} \cdot \frac{2023^2}{2022^2}
= \frac{2023}{2022^2}
\]

**Step 5: Final answer (exact)**

Plugging this in:

\[
-2022 \cdot \frac{2023}{2022^2} = -\frac{2023}{2022}
\]

**Step 6: Numerical value**

\[
2023/2022 \approx 1.0004945687
\]
So, the integral equals about \(-1.0004945687\)

---

**Final Answer in JSON Format:**
```json
{"answer": "-\\frac{2023}{2022}", "numerical_answer": "-1.0004945687"}
```