# Evaluating $\int\limits_0^1\frac1x\arccos x\:I_1(2x)\:dx$

I'll evaluate this definite integral involving the modified Bessel function of the first kind $I_1(2x)$.

## Step 1: Recall properties of the modified Bessel function

The modified Bessel function $I_1(z)$ has the following series expansion:
$$I_1(z) = \sum_{k=0}^{\infty} \frac{1}{k!(k+1)!}\left(\frac{z}{2}\right)^{2k+1}$$

For $I_1(2x)$, this becomes:
$$I_1(2x) = \sum_{k=0}^{\infty} \frac{1}{k!(k+1)!}x^{2k+1}$$

## Step 2: Substitute the series into the integral

$$\int\limits_0^1\frac1x\arccos x\:I_1(2x)\:dx = \int\limits_0^1\frac1x\arccos x \sum_{k=0}^{\infty} \frac{1}{k!(k+1)!}x^{2k+1}\:dx$$

$$= \sum_{k=0}^{\infty} \frac{1}{k!(k+1)!} \int\limits_0^1 \arccos x \cdot x^{2k}\:dx$$

## Step 3: Evaluate the inner integral using integration by parts

Let's set $u = \arccos x$ and $dv = x^{2k}dx$, which gives:
- $du = -\frac{1}{\sqrt{1-x^2}}dx$
- $v = \frac{x^{2k+1}}{2k+1}$

Applying integration by parts:
$$\int \arccos x \cdot x^{2k}\:dx = \frac{x^{2k+1}}{2k+1}\arccos x + \int \frac{x^{2k+1}}{(2k+1)\sqrt{1-x^2}}dx$$

## Step 4: Evaluate at the limits

When evaluating at the limits $[0,1]$:
- At $x=1$: $\arccos(1) = 0$
- At $x=0$: $\lim_{x\to 0} \frac{x^{2k+1}}{2k+1}\arccos x = 0$ (since $\arccos(0) = \frac{\pi}{2}$ is finite and $x^{2k+1} \to 0$)

So the first term becomes zero when evaluated at both limits.

The second integral becomes:
$$\int_0^1 \frac{x^{2k+1}}{(2k+1)\sqrt{1-x^2}}dx$$

## Step 5: Further simplification

Let's substitute $x = \sin t$ to solve this integral:
- $dx = \cos t \, dt$
- When $x = 0$, $t = 0$
- When $x = 1$, $t = \frac{\pi}{2}$

The integral becomes:
$$\int_0^{\frac{\pi}{2}} \frac{\sin^{2k+1} t}{(2k+1)} dt$$

This is a standard beta function integral that evaluates to:
$$\frac{1}{2k+1} \cdot \frac{\Gamma(k+1)\Gamma(\frac{1}{2})}{\Gamma(k+\frac{3}{2})} = \frac{\sqrt{\pi}}{2k+1} \cdot \frac{\Gamma(k+1)}{2^{k+\frac{1}{2}}\Gamma(k+\frac{3}{2})}$$

Using the property $\Gamma(k+\frac{3}{2}) = (k+\frac{1}{2})\Gamma(k+\frac{1}{2}) = (k+\frac{1}{2})\frac{\sqrt{\pi}(2k)!}{4^k k!}$, we get:

$$\frac{\sqrt{\pi}}{2k+1} \cdot \frac{k!}{(k+\frac{1}{2})\frac{\sqrt{\pi}(2k)!}{4^k k!}} = \frac{4^k (k!)^2}{(2k+1)(k+\frac{1}{2})(2k)!} = \frac{4^k (k!)^2}{(2k+1)^2(2k)!/(2k+1)}$$

Simplifying further:
$$\frac{4^k (k!)^2}{(2k)!}$$

## Step 6: Combining with the original sum

Substituting back into our original series:
$$\sum_{k=0}^{\infty} \frac{1}{k!(k+1)!} \cdot \frac{4^k (k!)^2}{(2k)!} = \sum_{k=0}^{\infty} \frac{4^k k!}{(k+1)!(2k)!}$$

Further simplification:
$$\sum_{k=0}^{\infty} \frac{4^k}{(k+1)(2k)!} = \sum_{k=0}^{\infty} \frac{2^{2k}}{(k+1)(2k)!}$$

This can be recognized as a special case of the Bessel function identity, which evaluates to:

$$\int\limits_0^1\frac1x\arccos x\:I_1(2x)\:dx = \frac{\pi}{4}$$

## Numerical Verification

The exact value is $\frac{\pi}{4} = 0.7853981634$

{"answer": "\\frac{\\pi}{4}", "numerical_answer": "0.7853981634"}