Let's compute the definite integral:
\[
I = \int_0^1 \frac{x-1}{(x+1)\ln x} \, dx
\]

## 1. Analytic Solution

### Step 1: Substitution

Notice that the derivative with respect to \(x\) of \(\ln(x+1)\) is \(\frac{1}{x+1}\), and also the denominator has \(\ln x\). 

Let us try to find a way to express the integrand, possibly via a parameter integral or as a derivative with respect to a parameter.

Write:
\[
\frac{x-1}{x+1} = 1 - \frac{2}{x+1}
\]
Thus,
\[
\int_0^1 \frac{x-1}{(x+1)\ln x} dx = \int_0^1 \frac{1}{\ln x} dx - 2 \int_0^1 \frac{1}{(x+1)\ln x} dx
\]
Let us call these terms \(I_1\) and \(I_2\):
\[
I_1 = \int_0^1 \frac{1}{\ln x} dx\,,\qquad I_2 = \int_0^1 \frac{1}{(x+1)\ln x} dx
\]

---

#### **Computing \(I_1 = \int_0^1 \frac{1}{\ln x}\,dx\) :**

We can use the standard result:
\[
\int_0^1 \frac{dx}{\ln x} = -\gamma
\]
where \(\gamma\) is the Euler–Mascheroni constant.

##### **Proof**:
Let \(J = \int_0^1 \frac{dx}{\ln x}\). Substitute \(x = e^{-y}\), so \(y = -\ln x\), as \(x\) goes from 0 to 1, \(y\) goes from \(\infty\) to 0:
\[
dx = -e^{-y} dy
\]
\[
J = \int_{y = \infty}^{y = 0} \frac{-e^{-y} dy}{-y} = \int_0^\infty \frac{e^{-y}}{y} dy
\]
This is the exponential integral \(\mathrm{Ei}(y)\) at \(\infty\), which gives Euler's constant:
\[
\int_0^1 \frac{dx}{\ln x} = -\int_0^\infty \frac{e^{-y}}{y} dy = -\gamma
\]

So,
\[
I_1 = -\gamma
\]

---

#### **Computing \(I_2 = \int_0^1 \frac{dx}{(x+1)\ln x}\) :**

Let us use the following representation:
\[
\frac{1}{x+1} = \int_0^\infty e^{-(x+1)t} dt = \int_0^\infty e^{-t} e^{-x t} dt
\]
Then,
\[
I_2 = \int_0^1 \frac{dx}{\ln x} \cdot \frac{1}{x+1} = \int_0^1 \frac{dx}{\ln x} \int_0^\infty e^{-t} e^{-x t} dt
\]
Switch order of integration (justification: Fubini-Tonelli because the integrand is non-negative for \(x \in (0,1)\), \(t > 0\)):
\[
I_2 = \int_0^\infty e^{-t} \left[\int_0^1 \frac{e^{-x t}}{\ln x} dx\right] dt
\]
Now, recall (integration formula):
\[
\int_0^1 x^{s-1} dx = \frac{1}{s}
\]
But that's not quite what we have. Instead, let's use a parameter trick. 

Note that:
\[
\int_0^1 x^{a} dx = \frac{1}{a+1}
\]
and
\[
\frac{d}{da} \int_0^1 x^a dx = \frac{d}{da} \left(\frac{1}{a+1}\right) = -\frac{1}{(a+1)^2}
\]
On the other hand,
\[
\frac{d}{da} \int_0^1 x^a dx = \int_0^1 x^a \ln x dx
\]
But we get:
\[
\int_0^1 x^a \ln x dx = -\frac{1}{(a+1)^2}
\]
Not exactly matching our form. Instead, let's note that for \(\text{Re}(s) > 0\), \(\int_0^1 x^{s-1} dx = \frac{1}{s}\). Now, 
\[
\int_0^1 x^{s-1} dx = \frac{1}{s}
\]
Let us try to relate our integral to logarithmic integrals.

Alternatively, we can use the expansion:
\[
\frac{1}{x+1} = \sum_{n=0}^\infty (-1)^n x^n
\]
for \(x \in (-1,1)\). For \(x \in [0,1]\), this series is absolutely convergent.

Therefore,
\[
I_2 = \int_0^1 \frac{1}{\ln x} \sum_{n=0}^\infty (-1)^n x^n dx = \sum_{n=0}^\infty (-1)^n \int_0^1 \frac{x^n}{\ln x} dx
\]

But
\[
\int_0^1 \frac{x^n}{\ln x} dx = -\int_0^1 x^n d x \ \text{(integration by parts)} 
\]
It is a standard result (see Gradshteyn & Ryzhik 4.231.1):
\[
\int_0^1 \frac{x^a - 1}{\ln x} dx = \psi(1) - \psi(a+1)
\]
But we only have \(x^a\):

Alternatively, here's a key well-known formula:
\[
\int_0^1 \frac{x^a}{\ln x} dx = -\frac{1}{a+1}
\]
(see Gradshteyn & Ryzhik 4.231.2).

This is because:
\[
\int_0^1 \frac{x^a}{\ln x} dx = \int_0^1 x^a \cdot \frac{1}{\ln x} dx
\]
But let's check this via substitution \(x = e^{-y}\), \(dx = -e^{-y} dy\), \(y = -\ln x\), \(x^a = e^{-a y}\). As \(x \to 0^+\), \(y\to\infty\), as \(x \to 1\), \(y\to 0\).
\[
\int_0^1 \frac{x^a}{\ln x} dx = \int_{y=\infty}^{y=0} \frac{e^{-a y}}{-y} \cdot (-e^{-y}) dy = \int_{0}^{\infty} \frac{e^{-(a+1)y}}{y} dy
\]
This is \(\text{Ei}(- (a+1)y)\) at infinity minus at 0, results in \(-\frac{1}{a+1}\).

So,
\[
\int_0^1 \frac{x^n}{\ln x} dx = -\frac{1}{n+1}
\]

Therefore,
\[
I_2 = \sum_{n=0}^\infty (-1)^n \left(-\frac{1}{n+1}\right) = \sum_{n=0}^\infty \frac{(-1)^{n+1}}{n+1}
\]
\[
= -\sum_{k=1}^\infty \frac{(-1)^k}{k}
\]

But the sum
\[
\sum_{k=1}^\infty \frac{(-1)^k}{k} = -\ln 2
\]
Therefore,
\[
I_2 = -(-\ln 2) = \ln 2
\]

---

### Step 2: Assemble the expression

Recall,
\[
I = I_1 - 2I_2 = -\gamma - 2\ln 2
\]

## 2. Numerical Approximation

Euler–Mascheroni constant: \(\gamma \approx 0.5772156649\)

\(\ln 2 \approx 0.6931471806\)

So,
\[
I \approx -0.5772156649 - 2 \times 0.6931471806 = -0.5772156649 - 1.3862943612 = -1.9635100261
\]

## 3. Final Answer

```json
{"answer": "-\\gamma - 2\\ln 2", "numerical_answer": "-1.9635100261"}
```