# Evaluating $\int_0^\pi\cos(x+\cos x)\:dx$

I'll solve this definite integral step-by-step.

## 1. Analyzing the integral

The integral is $\int_0^\pi\cos(x+\cos x)\:dx$. Let's make a substitution to simplify this.

Let $u = x + \cos x$, then:
$du = (1 - \sin x)\:dx$

Unfortunately, this substitution doesn't simplify our integral well because we can't easily express $dx$ in terms of $du$.

Let's try a different approach.

## 2. Using symmetry properties

Consider the function $f(x) = \cos(x+\cos x)$.

Let's examine what happens at $x$ and $\pi-x$:

At $x$: $f(x) = \cos(x+\cos x)$
At $\pi-x$: $f(\pi-x) = \cos(\pi-x+\cos(\pi-x)) = \cos(\pi-x-\cos(x)) = \cos(\pi-(x+\cos x)) = -\cos(x+\cos x) = -f(x)$

So we have $f(\pi-x) = -f(x)$, which means $f(x)$ is odd with respect to the point $\pi/2$.

## 3. Applying symmetry to the integral

For functions that are odd with respect to $\pi/2$ on the interval $[0,\pi]$, we know that:
$\int_0^\pi f(x)\:dx = 0$

This is because the contributions from $[0,\pi/2]$ and $[\pi/2,\pi]$ cancel each other out.

## 4. Verifying the result

Let's verify this by checking the integral:
$\int_0^\pi\cos(x+\cos x)\:dx = \int_0^{\pi/2}\cos(x+\cos x)\:dx + \int_{\pi/2}^{\pi}\cos(x+\cos x)\:dx$

Using our finding that $f(\pi-x) = -f(x)$, we can rewrite:
$\int_{\pi/2}^{\pi}\cos(x+\cos x)\:dx = -\int_{\pi/2}^{0}\cos((\pi-y)+\cos(\pi-y))\:(-dy)$
where $y = \pi-x$

This simplifies to:
$\int_{\pi/2}^{\pi}\cos(x+\cos x)\:dx = -\int_{0}^{\pi/2}\cos(y+\cos y)\:dy$

Therefore:
$\int_0^\pi\cos(x+\cos x)\:dx = \int_0^{\pi/2}\cos(x+\cos x)\:dx - \int_{0}^{\pi/2}\cos(x+\cos x)\:dx = 0$

## 5. Final answer

The exact value of the integral is:
$\int_0^\pi\cos(x+\cos x)\:dx = 0$

The numerical approximation, rounded to 10 decimal places, is:
$0.0000000000$

{"answer": "0", "numerical_answer": "0.0000000000"}