To solve the definite integral \(\int_{0}^{1} \arcsin(x) \arccos(x) \, dx\), we can follow these steps:

### Step 1: Simplify the Integrand
First, recall the relationship between \(\arcsin(x)\) and \(\arccos(x)\):
\[
\arcsin(x) + \arccos(x) = \frac{\pi}{2}
\]
Thus, we can express \(\arccos(x)\) as:
\[
\arccos(x) = \frac{\pi}{2} - \arcsin(x)
\]
Substituting this into the integrand:
\[
\arcsin(x) \arccos(x) = \arcsin(x) \left(\frac{\pi}{2} - \arcsin(x)\right) = \frac{\pi}{2} \arcsin(x) - \arcsin^2(x)
\]
So the integral becomes:
\[
\int_{0}^{1} \arcsin(x) \arccos(x) \, dx = \frac{\pi}{2} \int_{0}^{1} \arcsin(x) \, dx - \int_{0}^{1} \arcsin^2(x) \, dx
\]

### Step 2: Compute \(\int \arcsin(x) \, dx\)
We can compute \(\int \arcsin(x) \, dx\) using integration by parts:
Let \(u = \arcsin(x)\), \(dv = dx\). Then \(du = \frac{1}{\sqrt{1-x^2}} dx\), \(v = x\).
\[
\int \arcsin(x) \, dx = x \arcsin(x) - \int \frac{x}{\sqrt{1-x^2}} \, dx
\]
The second integral is:
\[
\int \frac{x}{\sqrt{1-x^2}} \, dx = -\sqrt{1-x^2} + C
\]
Thus:
\[
\int \arcsin(x) \, dx = x \arcsin(x) + \sqrt{1-x^2} + C
\]
Evaluating from 0 to 1:
\[
\left. x \arcsin(x) + \sqrt{1-x^2} \right|_{0}^{1} = \left(1 \cdot \frac{\pi}{2} + 0\right) - (0 + 1) = \frac{\pi}{2} - 1
\]

### Step 3: Compute \(\int \arcsin^2(x) \, dx\)
We can compute \(\int \arcsin^2(x) \, dx\) using integration by parts:
Let \(u = \arcsin^2(x)\), \(dv = dx\). Then \(du = \frac{2 \arcsin(x)}{\sqrt{1-x^2}} dx\), \(v = x\).
\[
\int \arcsin^2(x) \, dx = x \arcsin^2(x) - 2 \int \frac{x \arcsin(x)}{\sqrt{1-x^2}} \, dx
\]
For the second integral, let \(w = \arcsin(x)\), then \(dw = \frac{1}{\sqrt{1-x^2}} dx\), and \(x = \sin(w)\):
\[
\int \frac{x \arcsin(x)}{\sqrt{1-x^2}} \, dx = \int w \sin(w) \, dw
\]
Using integration by parts again:
Let \(a = w\), \(db = \sin(w) dw\). Then \(da = dw\), \(b = -\cos(w)\).
\[
\int w \sin(w) \, dw = -w \cos(w) + \int \cos(w) \, dw = -w \cos(w) + \sin(w) + C
\]
Substituting back \(w = \arcsin(x)\):
\[
\int \frac{x \arcsin(x)}{\sqrt{1-x^2}} \, dx = -\arcsin(x) \sqrt{1-x^2} + x + C
\]
Thus:
\[
\int \arcsin^2(x) \, dx = x \arcsin^2(x) - 2 \left(-\arcsin(x) \sqrt{1-x^2} + x\right) + C = x \arcsin^2(x) + 2 \arcsin(x) \sqrt{1-x^2} - 2x + C
\]
Evaluating from 0 to 1:
\[
\left. x \arcsin^2(x) + 2 \arcsin(x) \sqrt{1-x^2} - 2x \right|_{0}^{1} = \left(\frac{\pi^2}{4} + 0 - 2\right) - (0 + 0 - 0) = \frac{\pi^2}{4} - 2
\]

### Step 4: Combine the Results
Now, substitute the results back into the original expression:
\[
\int_{0}^{1} \arcsin(x) \arccos(x) \, dx = \frac{\pi}{2} \left(\frac{\pi}{2} - 1\right) - \left(\frac{\pi^2}{4} - 2\right) = \frac{\pi^2}{4} - \frac{\pi}{2} - \frac{\pi^2}{4} + 2 = 2 - \frac{\pi}{2}
\]

### Step 5: Numerical Approximation
The exact answer is \(2 - \frac{\pi}{2}\). Numerically:
\[
2 - \frac{\pi}{2} \approx 2 - 1.5707963268 = 0.4292036732
\]

### Final Answer
```json
{"answer": "2 - \\frac{\\pi}{2}", "numerical_answer": "0.4292036732"}
```