
To solve the definite integral \(\int_0^{\frac{\pi}{2}} x \ln(\sin x) \, dx\), we proceed as follows:

### Step 1: Series Expansion of \(\ln(\sin x)\)
The function \(\ln(\sin x)\) can be expressed using its Fourier series expansion for \(0 < x < \pi\):
\[
\ln(\sin x) = -\ln 2 - \sum_{n=1}^{\infty} \frac{\cos(2nx)}{n}
\]

### Step 2: Substitute the Series into the Integral
Substituting this series into the integral, we get:
\[
\int_0^{\frac{\pi}{2}} x \ln(\sin x) \, dx = \int_0^{\frac{\pi}{2}} x \left( -\ln 2 - \sum_{n=1}^{\infty} \frac{\cos(2nx)}{n} \right) dx
\]
This splits into two integrals:
\[
= -\ln 2 \int_0^{\frac{\pi}{2}} x \, dx - \sum_{n=1}^{\infty} \frac{1}{n} \int_0^{\frac{\pi}{2}} x \cos(2nx) \, dx
\]

### Step 3: Evaluate the First Integral
The first integral is straightforward:
\[
\int_0^{\frac{\pi}{2}} x \, dx = \left. \frac{x^2}{2} \right|_0^{\frac{\pi}{2}} = \frac{\pi^2}{8}
\]
Thus, the first term becomes:
\[
-\ln 2 \cdot \frac{\pi^2}{8}
\]

### Step 4: Evaluate the Second Integral (Term-by-Term)
For the second integral, we use integration by parts on \(\int x \cos(2nx) \, dx\). Let \(u = x\) and \(dv = \cos(2nx) \, dx\), so \(du = dx\) and \(v = \frac{\sin(2nx)}{2n}\). Applying integration by parts:
\[
\int x \cos(2nx) \, dx = \frac{x \sin(2nx)}{2n} + \frac{\cos(2nx)}{4n^2} + C
\]
Evaluating from \(0\) to \(\frac{\pi}{2}\):
\[
\left. \left( \frac{x \sin(2nx)}{2n} + \frac{\cos(2nx)}{4n^2} \right) \right|_0^{\frac{\pi}{2}} = \frac{\cos(n\pi)}{4n^2} - \frac{1}{4n^2} = \frac{(-1)^n - 1}{4n^2}
\]

### Step 5: Sum the Series
Substituting this result back into the second term:
\[
- \sum_{n=1}^{\infty} \frac{1}{n} \cdot \frac{(-1)^n - 1}{4n^2} = -\frac{1}{4} \sum_{n=1}^{\infty} \frac{(-1)^n - 1}{n^3}
\]
The series \(\sum_{n=1}^{\infty} \frac{(-1)^n - 1}{n^3}\) simplifies by noting that even \(n\) terms vanish (since \((-1)^n = 1\)), leaving only odd \(n\) terms:
\[
\sum_{n=1}^{\infty} \frac{(-1)^n - 1}{n^3} = -2 \sum_{k=1}^{\infty} \frac{1}{(2k-1)^3}
\]
Using the relation \(\zeta(3) = \sum_{n=1}^{\infty} \frac{1}{n^3} = \sum_{\text{odd } n} \frac{1}{n^3} + \sum_{\text{even } n} \frac{1}{n^3}\), we find \(\sum_{\text{odd } n} \frac{1}{n^3} = \frac{7}{8} \zeta(3)\). Thus:
\[
\sum_{n=1}^{\infty} \frac{(-1)^n - 1}{n^3} = -2 \cdot \frac{7}{8} \zeta(3) = -\frac{7}{4} \zeta(3)
\]
The second term becomes:
\[
-\frac{1}{4} \left( -\frac{7}{4} \zeta(3) \right) = \frac{7}{16} \zeta(3)
\]

### Step 6: Combine Results
Combining the two terms, the integral evaluates to:
\[
\int_0^{\frac{\pi}{2}} x \ln(\sin x) \, dx = -\frac{\pi^2}{8} \ln 2 + \frac{7}{16} \zeta(3)
\]

### Numerical Approximation
Using \(\pi \approx 3.141592653589793\), \(\ln 2 \approx 0.6931471805599453\), and \(\zeta(3) \approx 1.2020569031595943\):
\[
-\frac{\pi^2}{8} \ln 2 \approx -0.8551360496, \quad \frac{7}{16} \zeta(3) \approx 0.5258998951
\]
Adding these gives:
\[
-0.8551360496 + 0.5258998951 \approx -0.3292361545
\]

{"answer": "$-\\frac{\\pi^2}{8} \\ln 2 + \\frac{7}{16} \\zeta(3)$", "numerical_answer": "-0.3292361545"}