

To solve the definite integral \(\int_{0}^{1} \left( \frac{1}{x} - \left\lfloor \frac{1}{x} \right\rfloor \right) \, dx\), we proceed as follows:

### Step 1: Substitution
Let \( t = \frac{1}{x} \), so \( x = \frac{1}{t} \) and \( dx = -\frac{1}{t^2} dt \). When \( x \to 0^+ \), \( t \to \infty \), and when \( x = 1 \), \( t = 1 \). The integral transforms to:
\[
\int_{0}^{1} \left( \frac{1}{x} - \left\lfloor \frac{1}{x} \right\rfloor \right) dx = \int_{\infty}^{1} \left( t - \lfloor t \rfloor \right) \left( -\frac{1}{t^2} \right) dt = \int_{1}^{\infty} \frac{\{ t \}}{t^2} dt,
\]
where \( \{ t \} = t - \lfloor t \rfloor \) denotes the fractional part of \( t \).

### Step 2: Splitting the Integral
The fractional part \( \{ t \} \) satisfies \( \{ t \} = t - n \) for \( t \in [n, n+1) \) and integer \( n \geq 1 \). We split the integral into a sum over intervals \([n, n+1)\):
\[
\int_{1}^{\infty} \frac{\{ t \}}{t^2} dt = \sum_{n=1}^{\infty} \int_{n}^{n+1} \frac{t - n}{t^2} dt.
\]

### Step 3: Evaluating Each Integral
For each \( n \), compute the integral over \([n, n+1)\):
\[
\int_{n}^{n+1} \frac{t - n}{t^2} dt = \int_{n}^{n+1} \left( \frac{1}{t} - \frac{n}{t^2} \right) dt.
\]
Integrate term-by-term:
\[
\int_{n}^{n+1} \frac{1}{t} dt = \ln(t) \bigg|_{n}^{n+1} = \ln\left( \frac{n+1}{n} \right),
\]
\[
\int_{n}^{n+1} \frac{n}{t^2} dt = n \left( -\frac{1}{t} \right) \bigg|_{n}^{n+1} = n \left( \frac{1}{n} - \frac{1}{n+1} \right) = 1 - \frac{n}{n+1}.
\]
Thus, the integral over \([n, n+1)\) becomes:
\[
\ln\left( \frac{n+1}{n} \right) - \left( 1 - \frac{n}{n+1} \right) = \ln\left( \frac{n+1}{n} \right) - \frac{1}{n+1}.
\]

### Step 4: Summing the Series
The total integral is the sum over \( n \geq 1 \):
\[
\sum_{n=1}^{\infty} \left( \ln\left( \frac{n+1}{n} \right) - \frac{1}{n+1} \right).
\]
The first part of the sum telescopes:
\[
\sum_{n=1}^{\infty} \ln\left( \frac{n+1}{n} \right) = \lim_{N \to \infty} \ln(N+1).
\]
The second part is the harmonic series:
\[
\sum_{n=1}^{\infty} \frac{1}{n+1} = \lim_{N \to \infty} \left( H_{N+1} - 1 \right),
\]
where \( H_k \) is the \( k \)-th harmonic number. Using the asymptotic \( H_k \sim \ln k + \gamma \) (with \( \gamma \) the Euler-Mascheroni constant), we find:
\[
\lim_{N \to \infty} \left( \ln(N+1) - (H_{N+1} - 1) \right) = 1 - \gamma.
\]

### Exact and Numerical Results
The exact value of the integral is \( 1 - \gamma \). The Euler-Mascheroni constant \( \gamma \approx 0.5772156649015328606 \), so \( 1 - \gamma \approx 0.4227843350984671 \).

{"answer": "1 - \gamma", "numerical_answer": "0.4227843351"}