<think>
Okay, let's tackle this integral step by step. The integral is from 1/8 to 1/4 of [ln(2x) * ln(4x) * ln(8x)] / x dx. Hmm, that looks a bit complicated with three logarithmic terms multiplied together. I need to find a way to simplify this expression before integrating.

First, let me recall that when dealing with integrals involving multiple logarithms, substitution might be helpful. The denominator is x, which makes me think that substitution involving the logarithm could work here. Let's try to let u be something related to ln(x). Maybe if I set u = ln(x), then du = 1/x dx. That would take care of the 1/x term. Let's see.

But before that, maybe simplify the logarithms. Let's look at the arguments: 2x, 4x, 8x. Notice that 2x is 2*x, 4x is 4*x, and 8x is 8*x. These coefficients are powers of 2: 2^1, 2^2, 2^3. So maybe we can express each logarithm as ln(2^k * x) where k is 1, 2, 3. Let's write that out:

ln(2x) = ln(2) + ln(x)
ln(4x) = ln(4) + ln(x) = 2ln(2) + ln(x)
ln(8x) = ln(8) + ln(x) = 3ln(2) + ln(x)

So all three logarithms can be written as ln(2^k) + ln(x) for k=1,2,3. Let me substitute that into the original integrand:

[ (ln(2) + ln(x)) * (2ln(2) + ln(x)) * (3ln(2) + ln(x)) ] / x dx

So the integrand is the product of three linear terms in terms of ln(x) and constants involving ln(2). Let me denote t = ln(x) to simplify the expression. Then, the integrand becomes:

[ (ln(2) + t) * (2ln(2) + t) * (3ln(2) + t) ] * (1/x dx)

But since u = ln(x), then du = (1/x) dx. So the integral becomes:

∫ [ (ln(2) + u) * (2ln(2) + u) * (3ln(2) + u) ] du

But wait, the substitution is u = ln(x), so when x is 1/8, u = ln(1/8) = -3ln(2), and when x is 1/4, u = ln(1/4) = -2ln(2). So the limits of integration change from u = -3ln(2) to u = -2ln(2).

Therefore, the integral simplifies to:

∫ from u = -3ln(2) to u = -2ln(2) of [ (ln(2) + u) * (2ln(2) + u) * (3ln(2) + u) ] du

Now, let's expand the product inside the integral. Let me denote a = ln(2) for simplicity. Then the integrand becomes:

(a + u)(2a + u)(3a + u)

Let me first multiply the first two factors:

(a + u)(2a + u) = 2a² + a u + 2a u + u² = 2a² + 3a u + u²

Now multiply this result by the third factor (3a + u):

(2a² + 3a u + u²)(3a + u)

Let's expand term by term:

First term: 2a² * 3a = 6a³
Second term: 2a² * u = 2a² u
Third term: 3a u * 3a = 9a² u
Fourth term: 3a u * u = 3a u²
Fifth term: u² * 3a = 3a u²
Sixth term: u² * u = u³

Combine like terms:

6a³ + (2a² u + 9a² u) + (3a u² + 3a u²) + u³
= 6a³ + 11a² u + 6a u² + u³

So the integrand is 6a³ + 11a² u + 6a u² + u³, where a = ln(2). Therefore, the integral becomes:

∫_{-3a}^{-2a} [6a³ + 11a² u + 6a u² + u³] du

Now, let's integrate term by term.

First term: ∫6a³ du = 6a³ u

Second term: ∫11a² u du = 11a² * (u² / 2)

Third term: ∫6a u² du = 6a * (u³ / 3) = 2a u³

Fourth term: ∫u³ du = u⁴ / 4

So putting it all together, the antiderivative is:

6a³ u + (11a² / 2) u² + 2a u³ + (u⁴)/4

Now, we need to evaluate this from u = -3a to u = -2a.

Let's compute F(-2a) - F(-3a), where F(u) is the antiderivative.

First, compute F(-2a):

6a³*(-2a) + (11a² / 2)*(-2a)^2 + 2a*(-2a)^3 + (-2a)^4 /4

Compute each term:

1. 6a³*(-2a) = -12a⁴

2. (11a² / 2)*(4a²) = (11a² / 2)*4a² = 22a⁴

3. 2a*(-8a³) = -16a⁴

4. (16a⁴)/4 = 4a⁴

Adding these up: -12a⁴ +22a⁴ -16a⁴ +4a⁴ = (-12 +22 -16 +4)a⁴ = (-12 -16 +22 +4)a⁴ = (-28 +26)a⁴ = -2a⁴

Now compute F(-3a):

6a³*(-3a) + (11a² / 2)*(-3a)^2 + 2a*(-3a)^3 + (-3a)^4 /4

Compute each term:

1. 6a³*(-3a) = -18a⁴

2. (11a² / 2)*(9a²) = (99a⁴)/2

3. 2a*(-27a³) = -54a⁴

4. (81a⁴)/4

Adding these up:

-18a⁴ + (99/2)a⁴ -54a⁴ + (81/4)a⁴

Convert all terms to quarters to add:

-18a⁴ = -72/4 a⁴

(99/2)a⁴ = 198/4 a⁴

-54a⁴ = -216/4 a⁴

So total:

(-72/4 + 198/4 -216/4 +81/4) a⁴

Calculate numerator:

-72 +198 = 126; 126 -216 = -90; -90 +81 = -9

So total: (-9/4)a⁴

Therefore, F(-3a) = (-9/4)a⁴

Now, the definite integral is F(-2a) - F(-3a) = (-2a⁴) - (-9/4 a⁴) = (-2 + 9/4)a⁴ = (-8/4 +9/4)a⁴ = (1/4)a⁴

So the exact value of the integral is (1/4)(ln2)^4

Wait, let me check that again. Because a = ln2, so a⁴ = (ln2)^4, so the integral is (1/4)(ln2)^4.

But let me verify the calculations again to be sure.

First, F(-2a) was calculated as -2a⁴, and F(-3a) was -9/4 a⁴. Then, the difference: -2a⁴ - (-9/4 a⁴) = (-2 + 9/4)a⁴ = (1/4)a⁴. Yes, that's correct.

So the exact answer is (1/4)(ln2)^4. Let me write that in LaTeX: \frac{1}{4} (\ln 2)^4.

Now, for the numerical approximation. Let's compute (ln2)^4 first. ln2 is approximately 0.69314718056. Let's compute that to higher precision.

ln2 ≈ 0.6931471805599453

So (ln2)^4:

First, square ln2: 0.6931471805599453^2 ≈ 0.4804530139182014

Then square that: 0.4804530139182014^2 ≈ 0.4804530139182014 * 0.4804530139182014

Let me compute that:

0.48 * 0.48 = 0.2304

But more accurately:

0.4804530139182014 * 0.4804530139182014

Compute 0.4 * 0.4 = 0.16

0.4 * 0.4 = 0.16

But let's use a more precise method:

Let me compute 0.4804530139182014 * 0.4804530139182014:

First, write it as (0.4 + 0.0804530139182014)^2

= 0.4^2 + 2*0.4*0.0804530139182014 + (0.0804530139182014)^2

= 0.16 + 2*0.03218120556728056 + 0.0064727073746112

= 0.16 + 0.06436241113456112 + 0.0064727073746112

Adding up:

0.16 + 0.06436241113456112 = 0.22436241113456112

0.22436241113456112 + 0.0064727073746112 ≈ 0.2308351185091723

So (ln2)^4 ≈ 0.2308351185091723

Then multiply by 1/4: 0.2308351185091723 / 4 ≈ 0.057708779627293075

Rounded to 10 decimal places: 0.0577087796

Wait, let me check that division again. 0.2308351185 divided by 4:

0.2308351185 / 4 = 0.057708779625, so approximately 0.0577087796 when rounded to 10 decimal places.

Therefore, the numerical approximation is approximately 0.0577087796.

So the exact answer is (1/4)(ln2)^4, and the numerical value is approximately 0.0577087796.

Let me just confirm once more the steps. The substitution u = ln(x) transformed the integral into a polynomial in u, which was then integrated term by term. The limits were from -3ln2 to -2ln2, and after evaluating, the result simplified to (1/4)(ln2)^4. That seems correct. The key step was expanding the product of the three logarithms and then integrating term by term, which worked out nicely. I think this is correct.
</think>

{"answer": "\\frac{(\\ln 2)^4}{4}", "numerical_answer": "0.0577087796"}