Let's evaluate the integral:
\[
I = \int_0^\infty\frac{e^{-\frac{2019}{4t^2}}}{t^2}dt.
\]

**Step 1: Substitution**

Let \( a = \frac{2019}{4} \).

Make the substitution \( u = \frac{a}{t^2} \implies t = \sqrt{\frac{a}{u}} \).

Calculate \( dt \):

\[
t = (a/u)^{1/2} \implies dt = -\frac{1}{2} (a)^{1/2} u^{-3/2} du
\]

As \( t \rightarrow 0^+ \), \( u \rightarrow \infty \).
As \( t \rightarrow \infty \), \( u \rightarrow 0^+ \).

So:
\[
dt = -\frac{1}{2}a^{1/2}u^{-3/2}du
\]

Now rewrite the integrand: \( \frac{e^{-a/t^2}}{t^2} dt = e^{-u} \cdot \frac{1}{t^2} dt \)
But, \( t^2 = a/u \implies 1/t^2 = u/a \).

Therefore,
\[
I = \int_{t=0}^\infty \frac{e^{-a/t^2}}{t^2}dt = \int_{u=\infty}^{0} e^{-u}\frac{u}{a} \left(-\frac{1}{2}a^{1/2}u^{-3/2} du \right)
\]
Change limits and take the negative sign:
\[
= \int_{u=0}^\infty e^{-u}\frac{u}{a} \left(\frac{1}{2}a^{1/2}u^{-3/2} du \right)
\]

Simplifying:
\[
\frac{1}{a}\cdot\frac{1}{2}a^{1/2} \int_0^\infty e^{-u} u^{1-3/2} du
= \frac{1}{2a^{1/2}} \int_0^\infty e^{-u} u^{-1/2} du
\]
But, \( \int_0^\infty e^{-u} u^{-1/2} du = \Gamma(1/2) = \sqrt{\pi} \).

So,
\[
I = \frac{1}{2a^{1/2}} \sqrt{\pi}
\]
Recall \( a = \frac{2019}{4} \), thus \( a^{1/2} = \frac{\sqrt{2019}}{2} \):

\[
I = \frac{1}{2 \cdot \sqrt{2019}/2} \sqrt{\pi}
   = \frac{1}{\sqrt{2019}} \sqrt{\pi}
   = \sqrt{\frac{\pi}{2019}}
\]

**Step 2: Numerical Value**

\[
\sqrt{\frac{\pi}{2019}} \approx \sqrt{\frac{3.141592653589793}{2019}} \approx \sqrt{0.0015568031} \approx 0.0394663933
\]

**Step 3: Answer in JSON**

```json
{"answer": "\\sqrt{\\frac{\\pi}{2019}}", "numerical_answer": "0.0394663933"}
```