Let's compute the definite integral:
\[
I = \int_0^1 \left(\frac{x^2}{2-x^2} + \sqrt{\frac{2x}{x+1}}\right) dx
\]
We'll split the integral into two parts:
\[
I = I_1 + I_2
\]
where
\[
I_1 = \int_0^1 \frac{x^2}{2-x^2}dx, \quad I_2 = \int_0^1 \sqrt{\frac{2x}{x+1}}dx
\]

---

### Part 1: \( I_1 = \int_0^1 \frac{x^2}{2-x^2}dx \)

Rewriting:
\[
\frac{x^2}{2 - x^2} = \frac{2 - (2 - x^2)}{2-x^2} = 1 - \frac{2}{2-x^2}
\]
Therefore,
\[
I_1 = \int_0^1 1\,dx - 2\int_0^1 \frac{1}{2-x^2}dx
\]
So,
\[
I_1 = 1 - 2J, \quad \text{where } J = \int_0^1 \frac{1}{2-x^2}dx
\]

Now compute \( J \):

Note: \( \frac{1}{2-x^2} = \frac{1}{(\sqrt{2}-x)(\sqrt{2}+x)} \)

Partial fractions:
Let \[
\frac{1}{2-x^2} = \frac{A}{x-\sqrt{2}} + \frac{B}{x+\sqrt{2}}
\]
Compute \(A\) and \(B\):

\[
1 = A(x+\sqrt{2}) + B(x-\sqrt{2})
\]
Set \( x = \sqrt{2} \implies 1 = A(2\sqrt{2}), \; A = \frac{1}{2\sqrt{2}} \)

Set \( x = -\sqrt{2} \implies 1 = B(-2\sqrt{2}), \; B = -\frac{1}{2\sqrt{2}} \)

So,
\[
\frac{1}{2-x^2} = \frac{1}{2\sqrt{2}}\frac{1}{x-\sqrt{2}} - \frac{1}{2\sqrt{2}}\frac{1}{x+\sqrt{2}}
\]
Thus
\[
J = \int_0^1 \frac{1}{2-x^2}dx = \frac{1}{2\sqrt{2}}\int_0^1 \left(\frac{1}{x-\sqrt{2}}-\frac{1}{x+\sqrt{2}}\right)dx
\]

\[
=\frac{1}{2\sqrt{2}}\left(
\int_0^1 \frac{1}{x-\sqrt{2}}dx - \int_0^1 \frac{1}{x+\sqrt{2}}dx
\right)
\]

Integrate:
\[
\int \frac{1}{x-a} dx = \ln|x-a|
\]
So,
\[
J = \frac{1}{2\sqrt{2}}\left(
\left.\ln|x-\sqrt{2}|\right|_0^1 - \left.\ln|x+\sqrt{2}|\right|_0^1
\right)
\]
\[
= \frac{1}{2\sqrt{2}}\Big[
\ln|1-\sqrt{2}| - \ln|-\sqrt{2}| - \ln|1+\sqrt{2}| + \ln|\sqrt{2}|
\Big]
\]
\[
= \frac{1}{2\sqrt{2}}\Big[
(\ln|1-\sqrt{2}| - \ln|1+\sqrt{2}|) + (\ln|\sqrt{2}| - \ln|\sqrt{2}|) 
\Big]
\]
But \(\ln|-\sqrt{2}| = \ln|\sqrt{2}|\), so the last two cancel. Thus,

\[
J=\frac{1}{2\sqrt{2}}\left(\ln|1-\sqrt{2}|-\ln|1+\sqrt{2}|\right)
= \frac{1}{2\sqrt{2}}\ln\left|\frac{1-\sqrt{2}}{1+\sqrt{2}}\right|
\]

So,
\[
I_1 = 1 - 2J = 1 - \frac{1}{\sqrt{2}} \ln\left|\frac{1-\sqrt{2}}{1+\sqrt{2}}\right|
\]

---

### Part 2: \( I_2 = \int_0^1 \sqrt{\frac{2x}{x+1}}dx \)

Let’s write:
\[
I_2 = \int_0^1 \sqrt{2} \frac{\sqrt{x}}{\sqrt{x+1}} dx
\]

Let \( u = \sqrt{x} \), then \( x = u^2 \), \( dx = 2u\,du \).

When \( x=0 \), \( u=0 \), when \( x=1 \), \( u=1 \).

Transform the integral:
\[
I_2 = \sqrt{2} \int_0^1 \frac{u}{\sqrt{u^2+1}} 2u\,du = 2\sqrt{2} \int_0^1 \frac{u^2}{\sqrt{u^2+1}} du
\]

We can write \( u^2 = (u^2+1) - 1 \), so
\[
\frac{u^2}{\sqrt{u^2+1}} = \frac{u^2+1}{\sqrt{u^2+1}} - \frac{1}{\sqrt{u^2+1}} = \sqrt{u^2+1} - \frac{1}{\sqrt{u^2+1}}
\]

So now:
\[
I_2 = 2\sqrt{2} \int_0^1 \left( \sqrt{u^2+1} - \frac{1}{\sqrt{u^2+1}} \right) du
\]
\[
= 2\sqrt{2} \left( \int_0^1 \sqrt{u^2+1} du - \int_0^1 \frac{1}{\sqrt{u^2+1}} du \right )
\]

Recall:
\[
\int \sqrt{u^2+1} du = \frac{u}{2} \sqrt{u^2+1} + \frac{1}{2} \sinh^{-1}(u) + C
\]
\[
\int \frac{1}{\sqrt{u^2+1}} du = \sinh^{-1}(u) + C
\]

Therefore,
\[
I_2 = 2\sqrt{2} \left[
\left( \frac{u}{2} \sqrt{u^2+1} + \frac{1}{2} \sinh^{-1}u \right ) - \sinh^{-1}(u)
\right]_0^1
\]
\[
= 2\sqrt{2} \left[
\frac{u}{2} \sqrt{u^2+1} - \frac{1}{2} \sinh^{-1}u
\right]_0^1
\]
At \(u=1\), \( \sqrt{u^2+1} = \sqrt{2} \), \( \sinh^{-1}(1) = \ln(1+\sqrt{2}) \). At \(u=0\), both terms zero.

So,
\[
I_2 = 2\sqrt{2} \left( \frac{1}{2} \sqrt{2} - \frac{1}{2} \ln(1+\sqrt{2}) \right )
\]
\[
= 2\sqrt{2} \cdot \frac{1}{2} \left( \sqrt{2} - \ln(1+\sqrt{2}) \right )
\]
\[
= \sqrt{2} \left( \sqrt{2} - \ln(1+\sqrt{2}) \right )
\]
\[
= 2 - \sqrt{2} \ln(1+\sqrt{2})
\]

---

### Total Integral

\[
I = I_1 + I_2 = 1 - \frac{1}{\sqrt{2}}\ln\left|\frac{1-\sqrt{2}}{1+\sqrt{2}}\right| + 2 - \sqrt{2}\ln(1+\sqrt{2})
\]
\[
= 3 - \frac{1}{\sqrt{2}}\ln\left|\frac{1-\sqrt{2}}{1+\sqrt{2}}\right| - \sqrt{2}\ln(1+\sqrt{2})
\]

---

## Numerical Approximation

Let’s compute each part step by step:

- \( \sqrt{2} \approx 1.4142135623730951 \)
- \( 1-\sqrt{2} \approx -0.4142135623730951 \)
- \( 1+\sqrt{2} \approx 2.4142135623730951 \)
- \( \frac{1-\sqrt{2}}{1+\sqrt{2}} \approx -0.1715728752538097 \)
- \( \ln|1+\sqrt{2}| \approx \ln(2.4142135623730951) \approx 0.881373587019543 \)
- \( \ln|\frac{1-\sqrt{2}}{1+\sqrt{2}}| \approx \ln(0.1715728752538097) \approx -1.7640822121077216 \)

Now,

- \( \frac{1}{\sqrt{2}} \approx 0.7071067811865475 \)
- \( \frac{1}{\sqrt{2}}\ln\left|\frac{1-\sqrt{2}}{1+\sqrt{2}}\right| = 0.7071067811865475 \times (-1.7640822121077216) \approx -1.247435800117535 \)

- \( \sqrt{2}\ln(1+\sqrt{2}) = 1.4142135623730951 \times 0.881373587019543 \approx 1.246268656716024 \)

So,

\[
I \approx 3 - (-1.247435800117535) - 1.246268656716024
= 3 + 1.247435800117535 - 1.246268656716024
= 3 + (1.247435800117535 - 1.246268656716024)
= 3 + 0.001167143401511
= 3.001167143401511
\]

Rounded to 10 decimal places:

\[
I \approx 3.0011671434
\]

---

## JSON Output

```json
{"answer": "3 - \\frac{1}{\\sqrt{2}} \\ln\\left|\\frac{1-\\sqrt{2}}{1+\\sqrt{2}}\\right| - \\sqrt{2} \\ln(1+\\sqrt{2})", "numerical_answer": "3.0011671434"}
```