
To solve the definite integral \(\int_{0}^{2} x^{-1/2}(2 - x)^{-1/2}(1 + 0.5x)^{-2} T_2\left(\sqrt{1 + 0.5x}\right) \, dx\), we follow these steps:

### Step 1: Simplify the Chebyshev Polynomial
The second Chebyshev polynomial of the first kind is \(T_2(z) = 2z^2 - 1\). For \(z = \sqrt{1 + 0.5x}\), we have \(z^2 = 1 + 0.5x\), so:
\[
T_2\left(\sqrt{1 + 0.5x}\right) = 2(1 + 0.5x) - 1 = 1 + x.
\]

### Step 2: Rewrite the Integrand
Substituting \(T_2\left(\sqrt{1 + 0.5x}\right) = 1 + x\), the integrand becomes:
\[
x^{-1/2}(2 - x)^{-1/2}(1 + 0.5x)^{-2}(1 + x).
\]

### Step 3: Substitution to Simplify the Integral
Let \(x = 2\sin^2\theta\), so \(dx = 4\sin\theta\cos\theta \, d\theta\). When \(x = 0\), \(\theta = 0\); when \(x = 2\), \(\theta = \pi/2\). The terms \(x^{-1/2}(2 - x)^{-1/2}\) simplify to:
\[
x^{-1/2}(2 - x)^{-1/2} = \frac{1}{\sqrt{2}\sin\theta} \cdot \frac{1}{\sqrt{2}\cos\theta} = \frac{1}{2\sin\theta\cos\theta} = \frac{1}{\sin(2\theta)}.
\]
The term \(1 + 0.5x = 1 + \sin^2\theta\), so \((1 + 0.5x)^{-2} = (1 + \sin^2\theta)^{-2}\). The integrand transforms to:
\[
\frac{1}{\sin(2\theta)} \cdot (1 + \sin^2\theta)^{-2} \cdot (1 + 2\sin^2\theta) \cdot 4\sin\theta\cos\theta \, d\theta.
\]
Simplifying using \(\sin(2\theta) = 2\sin\theta\cos\theta\), the integrand reduces to:
\[
2 \cdot \frac{1 + 2\sin^2\theta}{(1 + \sin^2\theta)^2} \, d\theta.
\]

### Step 4: Evaluate the Integral
The integral becomes:
\[
2 \int_{0}^{\pi/2} \frac{1 + 2\sin^2\theta}{(1 + \sin^2\theta)^2} \, d\theta.
\]
Using trigonometric identities and integral tables, this evaluates to \(\frac{5\pi\sqrt{2}}{8}\).

### Step 5: Numerical Approximation
The numerical value of \(\frac{5\pi\sqrt{2}}{8}\) is approximately \(2.7768018178\) when rounded to 10 decimal places.

{"answer": "\\frac{5\\pi\\sqrt{2}}{8}", "numerical_answer": "2.7768018178"}