

To solve the definite integral \(\int_{420}^{1672}\frac{\sqrt{\ln(2023-x)}}{\sqrt{\ln(2023-x)}+\sqrt{\ln(x-69)}}\:\mathrm{d}x\), we use symmetry and substitution.

### Step 1: Identify Symmetry
Let \( f(x) = \frac{\sqrt{\ln(2023-x)}}{\sqrt{\ln(2023-x)}+\sqrt{\ln(x-69)}} \). Consider the substitution \( t = 2092 - x \), where \( 2092 = 420 + 1672 \) (the sum of the integration limits). This substitution flips the limits of integration: when \( x = 420 \), \( t = 1672 \), and when \( x = 1672 \), \( t = 420 \). Additionally, \( \mathrm{d}t = -\mathrm{d}x \), so the integral becomes:
\[
\int_{420}^{1672} f(x) \,\mathrm{d}x = \int_{1672}^{420} f(2092 - t) (-\mathrm{d}t) = \int_{420}^{1672} f(2092 - t) \,\mathrm{d}t.
\]

### Step 2: Simplify the Substituted Integrand
Simplify \( f(2092 - t) \):
- \( 2023 - (2092 - t) = t - 69 \), so \( \ln(2023 - (2092 - t)) = \ln(t - 69) \).
- \( (2092 - t) - 69 = 2023 - t \), so \( \ln((2092 - t) - 69) = \ln(2023 - t) \).

Thus, \( f(2092 - t) = \frac{\sqrt{\ln(t - 69)}}{\sqrt{\ln(t - 69)} + \sqrt{\ln(2023 - t)}} \).

### Step 3: Sum of Integrands
Notice that \( f(x) + f(2092 - x) = 1 \):
\[
f(x) + f(2092 - x) = \frac{\sqrt{\ln(2023-x)}}{\sqrt{\ln(2023-x)}+\sqrt{\ln(x-69)}} + \frac{\sqrt{\ln(x-69)}}{\sqrt{\ln(2023-x)}+\sqrt{\ln(x-69)}} = 1.
\]

### Step 4: Evaluate the Integral
Let \( I = \int_{420}^{1672} f(x) \,\mathrm{d}x \). By the substitution, \( I = \int_{420}^{1672} f(2092 - x) \,\mathrm{d}x \). Adding these:
\[
2I = \int_{420}^{1672} \left[ f(x) + f(2092 - x) \right] \,\mathrm{d}x = \int_{420}^{1672} 1 \,\mathrm{d}x = 1672 - 420 = 1252.
\]
Thus, \( I = \frac{1252}{2} = 626 \).

### Numerical Approximation
The exact value is an integer, so the numerical approximation is \( 626.0 \).

{"answer": "626", "numerical_answer": "626.0000000000"}