To solve the definite integral \(\int\limits_0^2 x H_{3}\left(\sqrt{x(2-x)}\right)dx\), where \(H_3\) is the third Hermite polynomial, we follow these steps:

### Step 1: Recall the Hermite Polynomial \(H_3(y)\)
The third Hermite polynomial is given by:
\[
H_3(y) = 8y^3 - 12y
\]
Thus, the integrand becomes:
\[
x H_3\left(\sqrt{x(2-x)}\right) = x \left[8\left(\sqrt{x(2-x)}\right)^3 - 12\sqrt{x(2-x)}\right]
\]
Simplify the expression:
\[
= 8x \left(x(2-x)\right)^{3/2} - 12x \left(x(2-x)\right)^{1/2}
\]

### Step 2: Simplify the Integral
The integral can be split into two parts:
\[
\int_0^2 x H_3\left(\sqrt{x(2-x)}\right)dx = 8 \int_0^2 x \left(x(2-x)\right)^{3/2} dx - 12 \int_0^2 x \left(x(2-x)\right)^{1/2} dx
\]

Let \(I_1 = \int_0^2 x \left(x(2-x)\right)^{3/2} dx\) and \(I_2 = \int_0^2 x \left(x(2-x)\right)^{1/2} dx\).

### Step 3: Use Substitution to Evaluate \(I_1\) and \(I_2\)
Let \(x = 2\sin^2\theta\), then \(dx = 4\sin\theta\cos\theta d\theta\), and the limits change from \(\theta = 0\) to \(\theta = \pi/2\).

For \(I_1\):
\[
I_1 = \int_0^{\pi/2} 2\sin^2\theta \left(2\sin^2\theta \cdot 2\cos^2\theta\right)^{3/2} \cdot 4\sin\theta\cos\theta d\theta
\]
Simplify:
\[
= 2 \cdot 8 \cdot 4 \int_0^{\pi/2} \sin^5\theta \cos^5\theta d\theta = 64 \int_0^{\pi/2} \sin^5\theta \cos^5\theta d\theta
\]
Using the identity \(\sin^5\theta \cos^5\theta = \frac{1}{32}\sin^5(2\theta)\), we get:
\[
I_1 = 64 \cdot \frac{1}{32} \int_0^{\pi/2} \sin^5(2\theta) d\theta = 2 \int_0^{\pi/2} \sin^5(2\theta) d\theta
\]
Let \(u = 2\theta\), then \(du = 2d\theta\), and the integral becomes:
\[
I_1 = \int_0^{\pi} \sin^5(u) \frac{du}{2} = \frac{1}{2} \int_0^{\pi} \sin^5(u) du
\]
The integral of \(\sin^5(u)\) over \([0, \pi]\) is \(\frac{16}{15}\), so:
\[
I_1 = \frac{1}{2} \cdot \frac{16}{15} = \frac{8}{15}
\]

For \(I_2\):
\[
I_2 = \int_0^{\pi/2} 2\sin^2\theta \left(2\sin^2\theta \cdot 2\cos^2\theta\right)^{1/2} \cdot 4\sin\theta\cos\theta d\theta
\]
Simplify:
\[
= 2 \cdot 2 \cdot 4 \int_0^{\pi/2} \sin^3\theta \cos^3\theta d\theta = 16 \int_0^{\pi/2} \sin^3\theta \cos^3\theta d\theta
\]
Using the identity \(\sin^3\theta \cos^3\theta = \frac{1}{8}\sin^3(2\theta)\), we get:
\[
I_2 = 16 \cdot \frac{1}{8} \int_0^{\pi/2} \sin^3(2\theta) d\theta = 2 \int_0^{\pi/2} \sin^3(2\theta) d\theta
\]
Let \(u = 2\theta\), then \(du = 2d\theta\), and the integral becomes:
\[
I_2 = \int_0^{\pi} \sin^3(u) \frac{du}{2} = \frac{1}{2} \int_0^{\pi} \sin^3(u) du
\]
The integral of \(\sin^3(u)\) over \([0, \pi]\) is \(\frac{4}{3}\), so:
\[
I_2 = \frac{1}{2} \cdot \frac{4}{3} = \frac{2}{3}
\]

### Step 4: Combine the Results
Now, substitute \(I_1\) and \(I_2\) back into the original expression:
\[
\int_0^2 x H_3\left(\sqrt{x(2-x)}\right)dx = 8 \cdot \frac{8}{15} - 12 \cdot \frac{2}{3} = \frac{64}{15} - 8 = \frac{64}{15} - \frac{120}{15} = -\frac{56}{15}
\]

### Step 5: Numerical Approximation
The numerical value of \(-\frac{56}{15}\) is approximately \(-3.7333333333\).

### Final Answer
```json
{"answer": "-\\frac{56}{15}", "numerical_answer": "-3.7333333333"}
```