
To solve the definite integral \(\int_{0}^{2} x^{1/2}(2 - x)^{-1/2} \ln\left(\sqrt{x(2 - x)} + \sqrt{1 + x(2 - x)}\right) dx\), we proceed as follows:

### Step 1: Simplify the Integrand
Let \( t = x(2 - x) \). The argument of the logarithm becomes \(\sqrt{t} + \sqrt{1 + t}\). Using the identity \(\sinh^{-1}(z) = \ln\left(z + \sqrt{z^2 + 1}\right)\), we recognize that:
\[
\ln\left(\sqrt{t} + \sqrt{1 + t}\right) = \sinh^{-1}\left(\sqrt{t}\right).
\]
Thus, the integral simplifies to:
\[
\int_{0}^{2} \sqrt{\frac{x}{2 - x}} \sinh^{-1}\left(\sqrt{x(2 - x)}\right) dx.
\]

### Step 2: Substitution
Let \( z = \sqrt{\frac{x}{2 - x}} \), so \( x = \frac{2z^2}{1 + z^2} \) and \( dx = \frac{4z}{(1 + z^2)^2} dz \). The limits \( x = 0 \) and \( x = 2 \) correspond to \( z = 0 \) and \( z \to \infty \), respectively. Substituting these into the integral, we find:
\[
\int_{0}^{\infty} z \cdot \sinh^{-1}\left(\frac{2z}{1 + z^2}\right) \cdot \frac{4z}{(1 + z^2)^2} dz.
\]

### Step 3: Differentiation Under the Integral Sign
Define \( I(a) = \int_{0}^{2} \sqrt{\frac{x}{2 - x}} \ln\left(a\sqrt{x(2 - x)} + \sqrt{1 + a^2 x(2 - x)}\right) dx \). We need \( I(1) \). Differentiating \( I(a) \) with respect to \( a \) and simplifying, we find:
\[
\frac{dI}{da} = \frac{2}{a} \arctan(a).
\]

### Step 4: Integrate to Find \( I(1) \)
Since \( I(0) = 0 \) (the logarithm term vanishes), we integrate \( \frac{dI}{da} \) from \( a = 0 \) to \( a = 1 \):
\[
I(1) = 2 \int_{0}^{1} \frac{\arctan(a)}{a} da.
\]
The integral \( \int_{0}^{1} \frac{\arctan(a)}{a} da \) is known to be Catalan's constant \( G \approx 0.915965594177 \). Thus:
\[
I(1) = 2G.
\]

### Numerical Approximation
Catalan's constant \( G \approx 0.915965594177 \), so \( 2G \approx 1.831931188354 \). Rounded to 10 decimal places, this is \( 1.8319311884 \).

### Final Answer
{"answer": "2G", "numerical_answer": "1.8319311884"}