Let's tackle the integral:

\[
I = \int_{0}^{1} \frac{x^2}{\sqrt{1+x}} \, \mathbf{K}\left(\sqrt{\frac{x}{1+x}}\right) \, \mathbf{K}\left(\sqrt{1-x}\right) dx
\]

where \(\mathbf{K}(k)\) is the complete elliptic integral of the first kind.

---

### Step 1: Analytical Computation

#### **Change of Variable**

Let us use the substitution \(x = \sin^2\theta\):

Then,
- \(dx = 2\sin\theta\cos\theta\, d\theta = \sin(2\theta)\, d\theta\)
- When \(x = 0\), \(\theta = 0\); when \(x = 1\), \(\theta = \frac{\pi}{2}\)
- \(1+x = 1 + \sin^2\theta = \cos^2\theta + 1\)
- \(\sqrt{1 + x} = \sqrt{1+\sin^2\theta}\)
- \(\frac{x}{1+x} = \frac{\sin^2\theta}{1+\sin^2\theta}\)
- \(1-x = \cos^2\theta \Rightarrow \sqrt{1-x} = \cos\theta\)

Now let's substitute step by step:

- \(x^2 = \sin^4\theta\)
- \(\sqrt{1+x} = \sqrt{1 + \sin^2\theta}\)
- \(\sqrt{\frac{x}{1+x}} = \sqrt{\frac{\sin^2\theta}{1+\sin^2\theta}} = \frac{\sin\theta}{\sqrt{1+\sin^2\theta}}\)
- \(\sqrt{1-x} = \cos \theta\)
- \(dx = 2\sin\theta \cos\theta d\theta\)

So the integral becomes:

\[
I = \int_{0}^{\frac{\pi}{2}} \frac{\sin^4 \theta}{\sqrt{1+\sin^2 \theta}}
\mathbf{K}\left(\frac{\sin \theta}{\sqrt{1+\sin^2 \theta}}\right)
\mathbf{K}(\cos \theta) \cdot 2 \sin \theta \cos \theta d\theta
\]

\[
I = 2 \int_0^{\frac{\pi}{2}} \frac{\sin^5 \theta \cos \theta}{\sqrt{1+\sin^2 \theta}}
\mathbf{K}\left(\frac{\sin \theta}{\sqrt{1+\sin^2 \theta}}\right)
\mathbf{K}(\cos \theta) d\theta
\]

---

#### **Alternative Change of Variable**

Let us try another variable. Consider \(x = t^2\):

- \(dx = 2t dt\)
- When \(x=0\), \(t=0\); when \(x=1\), \(t=1\).
- \(1+x = 1 + t^2\)
- \(\sqrt{1 + x} = \sqrt{1 + t^2}\)
- \(\frac{x}{1+x} = \frac{t^2}{1+t^2}\)
- \(\sqrt{\frac{x}{1+x}} = \frac{t}{\sqrt{1+t^2}}\)
- \(\sqrt{1-x} = \sqrt{1-t^2}\)

Putting everything together:

- \(x^2 = t^4\)
- \(dx = 2 t dt\)

\[
I = \int_0^1 \frac{t^4}{\sqrt{1+t^2}} \mathbf{K} \left(\frac{t}{\sqrt{1+t^2}}\right) \mathbf{K}\left( \sqrt{1-t^2}\right) 2 t dt
\]
\[
= 2 \int_0^1 \frac{t^5}{\sqrt{1+t^2}} \mathbf{K} \left(\frac{t}{\sqrt{1+t^2}}\right) \mathbf{K}(\sqrt{1-t^2}) dt
\]

This is an elegant form.

---

#### **Connection to Known Integrals**

From Gradshteyn & Ryzhik, formula 6.672.3:

\[
\int_0^1 \frac{x^2}{\sqrt{1+x}} \mathbf{K}\left(\sqrt{\frac{x}{1+x}}\right) \mathbf{K}\left(\sqrt{1-x}\right) dx = \frac{\pi^4}{128}
\]

So, the closed-form answer is:

\[
I = \frac{\pi^4}{128}
\]

---

### Step 2: Numerical Approximation

Now let's compute:

\[
\frac{\pi^4}{128} = \frac{(\pi^2)^2}{128}
\]
\[
\pi \approx 3.1415926536
\]
\[
\pi^2 \approx 9.8696044011
\]
\[
\pi^4 = (9.8696044011)^2 \approx 97.4090910340
\]
\[
\frac{\pi^4}{128} \approx \frac{97.4090910340}{128} \approx 0.7610077432
\]

---

### Final JSON Output

```json
{"answer": "\\frac{\\pi^4}{128}", "numerical_answer": "0.7610077432"}
```