Let's solve the given integral step by step.

### Given Integral:
\[
\int_{0}^{2.0} x^{1.0 - \frac{3}{2}} (2.0 - x)^{1.0 - \frac{1}{2}} \left[1 - 0.5x(2.0 - x)\right]^{-1.0} \, dx
\]

First, simplify the exponents and the integrand:
\[
\int_{0}^{2} x^{-\frac{1}{2}} (2 - x)^{\frac{1}{2}} \left[1 - \frac{1}{2}x(2 - x)\right]^{-1} \, dx
\]

Simplify the term inside the brackets:
\[
1 - \frac{1}{2}x(2 - x) = 1 - x + \frac{1}{2}x^2 = \frac{1}{2}(x^2 - 2x + 2)
\]
Thus, the integrand becomes:
\[
x^{-\frac{1}{2}} (2 - x)^{\frac{1}{2}} \left[\frac{1}{2}(x^2 - 2x + 2)\right]^{-1} = 2 x^{-\frac{1}{2}} (2 - x)^{\frac{1}{2}} (x^2 - 2x + 2)^{-1}
\]

Now, the integral is:
\[
2 \int_{0}^{2} \frac{(2 - x)^{\frac{1}{2}}}{x^{\frac{1}{2}} (x^2 - 2x + 2)} \, dx
\]

### Substitution:
Let \( x = 2 \sin^2 \theta \), then \( dx = 4 \sin \theta \cos \theta \, d\theta \). The limits change as follows:
- When \( x = 0 \), \( \theta = 0 \).
- When \( x = 2 \), \( \theta = \frac{\pi}{2} \).

Substitute \( x = 2 \sin^2 \theta \):
\[
2 - x = 2 \cos^2 \theta, \quad x^{\frac{1}{2}} = \sqrt{2} \sin \theta, \quad (2 - x)^{\frac{1}{2}} = \sqrt{2} \cos \theta
\]
The denominator \( x^2 - 2x + 2 \) becomes:
\[
(2 \sin^2 \theta)^2 - 2 \cdot 2 \sin^2 \theta + 2 = 4 \sin^4 \theta - 4 \sin^2 \theta + 2
\]
Simplify:
\[
4 \sin^4 \theta - 4 \sin^2 \theta + 2 = 2 (2 \sin^4 \theta - 2 \sin^2 \theta + 1)
\]

Now, the integral becomes:
\[
2 \int_{0}^{\frac{\pi}{2}} \frac{\sqrt{2} \cos \theta}{\sqrt{2} \sin \theta \cdot 2 (2 \sin^4 \theta - 2 \sin^2 \theta + 1)} \cdot 4 \sin \theta \cos \theta \, d\theta
\]
Simplify:
\[
2 \cdot \frac{\sqrt{2}}{\sqrt{2}} \cdot \frac{4}{2} \int_{0}^{\frac{\pi}{2}} \frac{\cos^2 \theta}{2 \sin^4 \theta - 2 \sin^2 \theta + 1} \, d\theta = 4 \int_{0}^{\frac{\pi}{2}} \frac{\cos^2 \theta}{2 \sin^4 \theta - 2 \sin^2 \theta + 1} \, d\theta
\]

### Further Simplification:
Let \( u = \sin \theta \), then \( du = \cos \theta \, d\theta \), and \( \cos^2 \theta = 1 - u^2 \). The integral becomes:
\[
4 \int_{0}^{1} \frac{1 - u^2}{2u^4 - 2u^2 + 1} \, du
\]

### Partial Fractions:
The denominator \( 2u^4 - 2u^2 + 1 \) can be factored as:
\[
2u^4 - 2u^2 + 1 = (u^2 + \sqrt{2}u + 1)(u^2 - \sqrt{2}u + 1)
\]
Thus, we can write:
\[
\frac{1 - u^2}{2u^4 - 2u^2 + 1} = \frac{A u + B}{u^2 + \sqrt{2}u + 1} + \frac{C u + D}{u^2 - \sqrt{2}u + 1}
\]
Solving for \( A, B, C, D \), we find:
\[
A = 0, \quad B = \frac{1}{2}, \quad C = 0, \quad D = \frac{1}{2}
\]
Thus:
\[
\frac{1 - u^2}{2u^4 - 2u^2 + 1} = \frac{1/2}{u^2 + \sqrt{2}u + 1} + \frac{1/2}{u^2 - \sqrt{2}u + 1}
\]

Now, the integral becomes:
\[
4 \cdot \frac{1}{2} \left[ \int_{0}^{1} \frac{1}{u^2 + \sqrt{2}u + 1} \, du + \int_{0}^{1} \frac{1}{u^2 - \sqrt{2}u + 1} \, du \right]
\]

### Evaluating the Integrals:
1. For \( \int \frac{1}{u^2 + \sqrt{2}u + 1} \, du \):
   Complete the square:
   \[
   u^2 + \sqrt{2}u + 1 = \left(u + \frac{\sqrt{2}}{2}\right)^2 + \frac{1}{2}
   \]
   Thus:
   \[
   \int \frac{1}{u^2 + \sqrt{2}u + 1} \, du = \sqrt{2} \arctan\left(\sqrt{2}u + 1\right)
   \]
   Evaluating from 0 to 1:
   \[
   \sqrt{2} \left[ \arctan(\sqrt{2} + 1) - \arctan(1) \right]
   \]

2. For \( \int \frac{1}{u^2 - \sqrt{2}u + 1} \, du \):
   Similarly:
   \[
   u^2 - \sqrt{2}u + 1 = \left(u - \frac{\sqrt{2}}{2}\right)^2 + \frac{1}{2}
   \]
   Thus:
   \[
   \int \frac{1}{u^2 - \sqrt{2}u + 1} \, du = \sqrt{2} \arctan\left(\sqrt{2}u - 1\right)
   \]
   Evaluating from 0 to 1:
   \[
   \sqrt{2} \left[ \arctan(\sqrt{2} - 1) - \arctan(-1) \right]
   \]

### Combining Results:
The integral becomes:
\[
2 \left[ \sqrt{2} \left( \arctan(\sqrt{2} + 1) - \arctan(1) + \arctan(\sqrt{2} - 1) - \arctan(-1) \right) \right]
\]
Simplify using \( \arctan(1) = \frac{\pi}{4} \) and \( \arctan(-1) = -\frac{\pi}{4} \):
\[
2 \sqrt{2} \left[ \arctan(\sqrt{2} + 1) + \arctan(\sqrt{2} - 1) \right]
\]
Using the identity \( \arctan a + \arctan b = \arctan\left(\frac{a + b}{1 - ab}\right) \) when \( ab < 1 \):
\[
\arctan(\sqrt{2} + 1) + \arctan(\sqrt{2} - 1) = \arctan\left(\frac{2\sqrt{2}}{0}\right) = \frac{\pi}{2}
\]
Thus:
\[
2 \sqrt{2} \cdot \frac{\pi}{2} = \sqrt{2} \pi
\]

### Numerical Approximation:
\[
\sqrt{2} \pi \approx 4.4428829381
\]

### Final Answer:
```json
{"answer": "\\sqrt{2} \\pi", "numerical_answer": "4.4428829381"}
```