<think>
Okay, let's see. I need to compute the definite integral from 0 to 2 of x^(-1/2)(2 - x)^(1/2)[1 - 0.5x(2 - x)]^(1/2) dx. Hmm, that looks a bit complicated. Let me break it down step by step.

First, let me rewrite the integrand to make it clearer. The integrand is x^{-1/2} * (2 - x)^{1/2} * [1 - 0.5x(2 - x)]^{1/2}. Maybe simplifying the expression inside the square roots would help. Let's look at the term inside the third factor: 1 - 0.5x(2 - x). Let me expand that.

0.5x(2 - x) = 0.5*(2x - x²) = x - 0.5x². So, 1 - (x - 0.5x²) = 1 - x + 0.5x². So the integrand becomes x^{-1/2} * (2 - x)^{1/2} * sqrt(1 - x + 0.5x²). Hmm, not sure if that helps yet.

Alternatively, maybe a substitution would be useful here. Let's consider substitution variables. The limits are from 0 to 2, so maybe a substitution that maps 0 to 2 into a symmetric interval or something. Let me think about trigonometric substitutions. For integrals involving sqrt(a - x) and sqrt(x), sometimes substituting x = a sin²θ or something similar works. Let's try that.

Let me set x = 2 sin²θ. Then, when x=0, θ=0, and when x=2, θ=π/2. Let's compute dx: dx = 4 sinθ cosθ dθ. Now, let's substitute into the integrand.

First, x^{-1/2} = (2 sin²θ)^{-1/2} = (2)^{-1/2} (sinθ)^{-1}.

Next, (2 - x)^{1/2} = (2 - 2 sin²θ)^{1/2} = (2 cos²θ)^{1/2} = sqrt(2) cosθ.

Then, the third term: [1 - 0.5x(2 - x)]^{1/2}. Let's compute 0.5x(2 - x). Substituting x = 2 sin²θ, we get 0.5*(2 sin²θ)*(2 - 2 sin²θ) = 0.5*2 sin²θ*2 cos²θ = 2 sin²θ cos²θ. Therefore, 1 - 0.5x(2 - x) = 1 - 2 sin²θ cos²θ. Hmm, maybe simplify that expression.

Wait, 2 sin²θ cos²θ is equal to (sin²2θ)/2, since sin2θ = 2 sinθ cosθ, so sin²2θ = 4 sin²θ cos²θ, so 2 sin²θ cos²θ = (sin²2θ)/2. Therefore, 1 - 2 sin²θ cos²θ = 1 - (sin²2θ)/2. Hmm, not sure if that helps. Alternatively, maybe use double-angle identities.

Alternatively, let's compute 1 - 2 sin²θ cos²θ. Let me see: 1 - 2 sin²θ cos²θ = 1 - (1/2)(2 sinθ cosθ)^2 = 1 - (1/2) sin²2θ. So sqrt(1 - (1/2) sin²2θ). Hmm, that's sqrt(1 - (1/2) sin²2θ). That looks like an elliptic integral? Because integrals involving sqrt(1 - k² sin²θ) are elliptic integrals. Wait, but maybe there's a way to simplify this.

Alternatively, maybe another substitution. Let me check the entire integrand after substitution. Let's put all the substituted terms together.

Original integrand after substitution:

x^{-1/2} * (2 - x)^{1/2} ) * [1 - 0.5x(2 - x)]^{1/2} dx

Substituted:

(2^{-1/2} sin^{-1}θ) * (sqrt(2) cosθ) * sqrt(1 - 2 sin²θ cos²θ) * 4 sinθ cosθ dθ

Let's compute each part:

First term: 2^{-1/2} * sin^{-1}θ

Second term: sqrt(2) cosθ

Third term: sqrt(1 - 2 sin²θ cos²θ)

Fourth term: 4 sinθ cosθ dθ

Multiply them all together:

2^{-1/2} * sqrt(2) = 2^{-1/2 + 1/2} = 2^0 = 1

Then, sin^{-1}θ * cosθ * 4 sinθ cosθ = 4 cos²θ

So, the integrand simplifies to 4 cos²θ * sqrt(1 - 2 sin²θ cos²θ) dθ

Wait, let me check that again:

Original substitution:

x = 2 sin²θ, dx = 4 sinθ cosθ dθ

x^{-1/2} = (2 sin²θ)^{-1/2} = 2^{-1/2} sin^{-1}θ

(2 - x)^{1/2} = sqrt(2 - 2 sin²θ) = sqrt(2 cos²θ) = sqrt(2) cosθ

[1 - 0.5x(2 - x)]^{1/2} = sqrt(1 - 0.5*2 sin²θ*2 cos²θ) = sqrt(1 - 2 sin²θ cos²θ)

Multiply all together:

2^{-1/2} * sin^{-1}θ * sqrt(2) cosθ * sqrt(1 - 2 sin²θ cos²θ) * 4 sinθ cosθ dθ

Simplify constants:

2^{-1/2} * sqrt(2) = 1

sin^{-1}θ * sinθ = 1

cosθ * cosθ = cos²θ

So, 1 * 1 * cos²θ * sqrt(1 - 2 sin²θ cos²θ) * 4 dθ

So the integrand becomes 4 cos²θ sqrt(1 - 2 sin²θ cos²θ) dθ

Hmm, that's still complicated. Let me see if I can simplify the expression under the square root.

1 - 2 sin²θ cos²θ. Let's note that sin²θ cos²θ = (1/4) sin²2θ. So 1 - 2*(1/4) sin²2θ = 1 - (1/2) sin²2θ. Therefore, sqrt(1 - (1/2) sin²2θ). So the integrand is 4 cos²θ sqrt(1 - (1/2) sin²2θ) dθ.

Hmm, maybe another substitution. Let me set φ = 2θ. Then, when θ = 0, φ = 0; when θ = π/2, φ = π. But the upper limit would be π, but maybe that's not helpful. Alternatively, perhaps use a different substitution.

Alternatively, note that the integrand is 4 cos²θ sqrt(1 - (1/2) sin²2θ) dθ. Let's express cos²θ in terms of double angles. cos²θ = (1 + cos2θ)/2. So substituting that in:

4 * (1 + cos2θ)/2 * sqrt(1 - (1/2) sin²2θ) dθ = 2(1 + cos2θ) sqrt(1 - (1/2) sin²2θ) dθ

Hmm, maybe set φ = 2θ. Then, dφ = 2 dθ, so dθ = dφ/2. When θ=0, φ=0; θ=π/2, φ=π. Then, the integral becomes:

2 * (1 + cosφ) * sqrt(1 - (1/2) sin²φ) * (dφ/2) integrated from 0 to π.

Simplify constants: 2 * (1/2) = 1. So the integral is ∫ from 0 to π (1 + cosφ) sqrt(1 - (1/2) sin²φ) dφ.

Hmm, that's an integral from 0 to π. Let's split the integral into two parts: ∫ (1 + cosφ) sqrt(...) dφ = ∫ sqrt(...) dφ + ∫ cosφ sqrt(...) dφ.

But I'm not sure if that helps. Alternatively, note that sqrt(1 - (1/2) sin²φ) is similar to the form of elliptic integrals. The standard elliptic integral of the second kind is E(φ, k) = ∫ sqrt(1 - k² sin²θ) dθ. But here, we have sqrt(1 - (1/2) sin²φ), so k² = 1/2, so k = 1/√2. But the integral here is multiplied by (1 + cosφ). Hmm.

Alternatively, maybe use symmetry. The integral from 0 to π can be split into 0 to π/2 and π/2 to π. Let me see if there's a substitution for the second half. Let φ = π - t in the second integral. Then, when φ = π/2, t = π/2; when φ=π, t=0. Then, cosφ = cos(π - t) = -cos t, sinφ = sin(π - t) = sin t. So the integral from π/2 to π becomes ∫ from π/2 to 0 (1 - cos t) sqrt(1 - (1/2) sin²t) (-dt) = ∫ from 0 to π/2 (1 - cos t) sqrt(1 - (1/2) sin²t) dt.

Therefore, the original integral becomes ∫0^{π/2} (1 + cosφ) sqrt(...) dφ + ∫0^{π/2} (1 - cosφ) sqrt(...) dφ = ∫0^{π/2} [ (1 + cosφ) + (1 - cosφ) ] sqrt(1 - (1/2) sin²φ) dφ = ∫0^{π/2} 2 sqrt(1 - (1/2) sin²φ) dφ.

So the integral simplifies to 2 ∫0^{π/2} sqrt(1 - (1/2) sin²φ) dφ. That's 2 times the elliptic integral of the second kind E(1/√2). Wait, the standard form is E(k) = ∫0^{π/2} sqrt(1 - k² sin²θ) dθ. So here, k² = 1/2, so k = 1/√2. Therefore, the integral is 2 E(1/√2).

But the problem says to compute the integral analytically. If it's an elliptic integral, then maybe that's the answer. But I need to check if there's a way to express this in terms of known constants or simpler functions. However, elliptic integrals are considered special functions and might be acceptable as an exact answer. Let me confirm.

Alternatively, maybe there's a substitution that can convert the original integral into a Beta function or Gamma function. Let me revisit the original integral.

Original integral: ∫0^2 x^{-1/2} (2 - x)^{1/2} [1 - 0.5x(2 - x)]^{1/2} dx.

Let me make a substitution t = x/2, so x = 2t, dx = 2dt. Then, the limits become t=0 to t=1.

Substituting, we get:

∫0^1 (2t)^{-1/2} (2 - 2t)^{1/2} [1 - 0.5*(2t)(2 - 2t)]^{1/2} * 2 dt

Simplify each term:

(2t)^{-1/2} = (2)^{-1/2} t^{-1/2}

(2 - 2t)^{1/2} = (2(1 - t))^{1/2} = sqrt(2) (1 - t)^{1/2}

[1 - 0.5*(2t)(2 - 2t)] = 1 - 0.5*(4t(1 - t)) = 1 - 2t(1 - t) = 1 - 2t + 2t²

So the integrand becomes:

2^{-1/2} t^{-1/2} * sqrt(2) (1 - t)^{1/2} * sqrt(1 - 2t + 2t²) * 2 dt

Simplify constants:

2^{-1/2} * sqrt(2) = 1, and multiplied by 2 gives 2.

So the integral becomes 2 ∫0^1 t^{-1/2} (1 - t)^{1/2} sqrt(1 - 2t + 2t²) dt

Hmm, the term sqrt(1 - 2t + 2t²) can be rewritten as sqrt(2t² - 2t + 1). Let's see if that quadratic can be expressed in a different form. 2t² - 2t + 1 = 2(t² - t) + 1 = 2(t² - t + 1/4) + 1 - 2*(1/4) = 2(t - 1/2)^2 + 1 - 1/2 = 2(t - 1/2)^2 + 1/2. So sqrt(2(t - 1/2)^2 + 1/2). Not sure if that helps.

Alternatively, maybe another substitution. Let me set u = t - 1/2. Then, t = u + 1/2, dt = du. The limits when t=0, u=-1/2; t=1, u=1/2. The integral becomes:

2 ∫_{-1/2}^{1/2} (u + 1/2)^{-1/2} (1 - (u + 1/2))^{1/2} sqrt(2u² + 1/2) du

Simplify the terms:

(1 - (u + 1/2)) = (1/2 - u) = (1/2 - u). So (1/2 - u)^{1/2}

So the integrand is:

(u + 1/2)^{-1/2} (1/2 - u)^{1/2} sqrt(2u² + 1/2) du

Hmm, this seems more complicated. Maybe this substitution isn't helpful. Let's think differently.

Looking back at the integral after substitution t = x/2, we have:

2 ∫0^1 t^{-1/2} (1 - t)^{1/2} sqrt(1 - 2t + 2t²) dt

The term t^{-1/2} (1 - t)^{1/2} is similar to the Beta function integrand, which is t^{c-1} (1 - t)^{d - c -1}, but here we have an extra sqrt(1 - 2t + 2t²) term. Maybe this integral can be expressed in terms of hypergeometric functions or other special functions. Alternatively, perhaps there's a connection to elliptic integrals.

Alternatively, let's consider that the original substitution led us to an elliptic integral. If the integral reduces to 2 E(1/√2), then that's the exact answer. Let me check the steps again to confirm.

Earlier steps:

Original integral after substitution x = 2 sin²θ became 4 cos²θ sqrt(1 - (1/2) sin²2θ) dθ from 0 to π/2. Then, after splitting the integral and using substitution, it simplified to 2 ∫0^{π/2} sqrt(1 - (1/2) sin²φ) dφ. Which is 2 E(1/√2). So the exact answer is 2 times the elliptic integral of the second kind with modulus k = 1/√2.

But I need to confirm if this is correct. Let me verify with a different approach.

Alternatively, let's consider the integral ∫0^2 x^{-1/2} (2 - x)^{1/2} sqrt(1 - 0.5x(2 - x)) dx.

Let me denote the integral as I. Let me make substitution y = x/2, so x = 2y, dx = 2dy, limits from 0 to 1.

Then, I = ∫0^1 (2y)^{-1/2} (2 - 2y)^{1/2} sqrt(1 - 0.5*(2y)(2 - 2y)) * 2 dy

Simplify:

(2y)^{-1/2} = (2)^{-1/2} y^{-1/2}

(2 - 2y)^{1/2} = (2)^{1/2} (1 - y)^{1/2}

sqrt(1 - 0.5*(2y)(2 - 2y)) = sqrt(1 - 0.5*(4y - 4y²)) = sqrt(1 - 2y + 2y²)

Multiply all together:

(2)^{-1/2} * (2)^{1/2} = 1

y^{-1/2} (1 - y)^{1/2} sqrt(1 - 2y + 2y²) * 2 dy

So I = 2 ∫0^1 y^{-1/2} (1 - y)^{1/2} sqrt(1 - 2y + 2y²) dy

Hmm, this seems similar to the previous expression. Let me check if this can be expressed in terms of Beta functions or Gamma functions. The term y^{-1/2} (1 - y)^{1/2} is part of the Beta function B(1/2, 3/2), but multiplied by sqrt(1 - 2y + 2y²). Not sure.

Alternatively, maybe expand sqrt(1 - 2y + 2y²) in a series and integrate term by term. But that might be complicated. Alternatively, note that 1 - 2y + 2y² = 2y² - 2y + 1 = 2(y² - y) + 1. Completing the square: y² - y = (y - 1/2)^2 - 1/4. So 2(y - 1/2)^2 - 1/2 + 1 = 2(y - 1/2)^2 + 1/2. So sqrt(2(y - 1/2)^2 + 1/2). This is similar to sqrt(a^2 + b^2(y - c)^2), which might relate to elliptic integrals, but I'm not sure.

Alternatively, perhaps use a substitution z = y - 1/2. Then, y = z + 1/2, dy = dz. The limits become z = -1/2 to z = 1/2. The integral becomes:

2 ∫_{-1/2}^{1/2} (z + 1/2)^{-1/2} (1 - (z + 1/2))^{1/2} sqrt(2z² + 1/2) dz

Simplify:

(1 - (z + 1/2)) = (1/2 - z) = (1/2 - z)^{1/2}

So the integrand is:

(z + 1/2)^{-1/2} (1/2 - z)^{1/2} sqrt(2z² + 1/2) dz

Hmm, this still looks complicated. Maybe this isn't the right path.

Going back to the previous result where the integral reduces to 2 E(1/√2). Let me check if that's correct. The elliptic integral of the second kind E(k) is defined as ∫0^{π/2} sqrt(1 - k² sin²θ) dθ. In our case, after substitution, we have 2 ∫0^{π/2} sqrt(1 - (1/2) sin²φ) dφ = 2 E(1/√2). So the exact answer is 2 E(1/√2). 

But how to express this in terms of known constants? The exact value of E(1/√2) is known in terms of Gamma functions. There is a formula for E(k) when k = 1/√2. Specifically, for the case where the modulus k is 1/√2, which is a common case. 

The complete elliptic integral of the second kind E(k) can be expressed using the Gamma function. The formula is:

E(1/√2) = [Gamma(1/4) Gamma(3/4)]/(4 sqrt(2π)) + [sqrt(2π) Gamma(3/4)^2]/(4 Gamma(1/4))

But I might be misremembering. Alternatively, there's a relation when m = k² = 1/2. 

From the Legendre relation, for complementary modulus, but perhaps that's helpful here. Alternatively, using the formula:

E(1/√2) = [sqrt(2)/4] * [Gamma(1/4)]^2 / sqrt(π)

Wait, let me check known values. The complete elliptic integral of the second kind E(k) for k = sin(π/8) or k = 1/√2. 

According to some references, E(1/√2) can be expressed as:

E(1/√2) = (sqrt(2)/4) * [Gamma(1/4)]^2 / sqrt(π) + [sqrt(π/2)/4] * [Gamma(1/4)]^2 / Gamma(3/4)^2

Wait, this seems complicated. Alternatively, using the relation between Gamma functions:

It's known that Gamma(1/4) Gamma(3/4) = π*sqrt(2). So, Gamma(1/4) Gamma(3/4) = π*sqrt(2). Therefore, E(1/√2) can be written in terms of Gamma(1/4). 

From the formula for E(k), when k = 1/√2, we have:

E(1/√2) = [Gamma(1/4)^2 + 2π^{3/2}]/(4 sqrt(2π))}

Wait, I need to verify this. Alternatively, according to some sources, E(1/√2) = (sqrt(2)/4) * [Gamma(1/4)]^2 / sqrt(π). Let me check this.

Using the formula for E(k):

E(k) = (π/2) * [1 - (1/2)^2/(1) * k² - (1*3/2*4)^2/(3) * k^4 - ... ]

But this series might not help here. Alternatively, using the relation between Beta and Gamma functions. The integral E(k) can be expressed as:

E(k) = (π/2) * 2F1(-1/2, 1/2; 1; k²)

But hypergeometric functions might not be helpful here. Alternatively, using the relation:

E(1/√2) = [sqrt(2)/4] * [Gamma(1/4)]^2 / sqrt(π)

Let me compute this. If Gamma(1/4) ≈ 3.6256099082, then [Gamma(1/4)]^2 ≈ (3.6256)^2 ≈ 13.145. Then sqrt(2)/4 * 13.145 / sqrt(π) ≈ 1.4142/4 * 13.145 / 1.77245 ≈ 0.35355 * 13.145 / 1.77245 ≈ 4.65 / 1.77245 ≈ 2.62. But the actual value of E(1/√2) is approximately 1.350643881. So this formula might not be correct.

Alternatively, perhaps E(1/√2) = [Gamma(1/4)]^2/(4 sqrt(2π)) + sqrt(π/2)/2. Let me check:

Gamma(1/4) ≈ 3.62561

[Gamma(1/4)]^2 ≈ 13.145

13.145 / (4 * sqrt(2π)) ≈ 13.145 / (4 * 2.5066) ≈ 13.145 / 10.0264 ≈ 1.31

sqrt(π/2)/2 ≈ 1.2533 / 2 ≈ 0.6267

Adding them gives 1.31 + 0.6267 ≈ 1.9367, which is not matching the known value. So perhaps that's not the right formula.

Alternatively, perhaps I should just accept that the exact value is 2 E(1/√2) and provide that as the exact answer. Since the problem says to compute the integral analytically, and elliptic integrals are standard special functions, this might be acceptable.

Therefore, the exact answer is 2 E(1/√2). For the numerical approximation, I can look up the value of E(1/√2). 

Looking up the value of the complete elliptic integral of the second kind E(k) for k = 1/√2. According to mathematical references, E(1/√2) ≈ 1.350643881. Therefore, multiplying by 2 gives approximately 2.701287762. Rounded to 10 decimal places, that's 2.7012877620.

But let me verify this with a calculator or computational tool. Using Wolfram Alpha, for example, the integral ∫0^2 x^{-1/2} (2 - x)^{1/2} sqrt(1 - 0.5x(2 - x)) dx. 

Alternatively, compute 2*EllipticE(1/√2). Let me check:

EllipticE(1/√2) is approximately 1.350643881, so 2*1.350643881 ≈ 2.701287762. Rounded to 10 decimal places, 2.7012877620.

Therefore, the exact answer is 2 E(1/√2), which can be written in LaTeX as 2\,E\left(\frac{1}{\sqrt{2}}\right), and the numerical approximation is approximately 2.7012877620.
</think>

{"answer": "2\\,E\\left(\\frac{1}{\\sqrt{2}}\\right)", "numerical_answer": "2.7012877620"}