To solve the definite integral \(\int_{-4}^4 e^{|x|} \cdot \{x\} \, dx\), where \(\{x\}\) denotes the fractional part of \(x\), we follow these steps:

### Step 1: Understand the Fractional Part Function
The fractional part of \(x\), denoted \(\{x\}\), is defined as:
\[
\{x\} = x - \lfloor x \rfloor
\]
where \(\lfloor x \rfloor\) is the floor function (the greatest integer less than or equal to \(x\)).

### Step 2: Break the Integral into Intervals
The fractional part function \(\{x\}\) is periodic with period 1. Therefore, we can break the integral into unit intervals where the fractional part behaves uniformly. However, since the integral is from \(-4\) to \(4\), we consider the intervals where \(\{x\}\) changes its behavior:

For \(x \in [-4, 0)\):
\[
\{x\} = x - \lfloor x \rfloor = x - (-4) = x + 4 \quad \text{for } x \in [-4, -3)
\]
Similarly, we can write \(\{x\}\) for each interval \([-n, -n+1)\) for \(n = 4, 3, 2, 1\).

For \(x \in [0, 4)\):
\[
\{x\} = x - \lfloor x \rfloor = x \quad \text{for } x \in [0, 1)
\]
and similarly for each interval \([n, n+1)\) for \(n = 0, 1, 2, 3\).

### Step 3: Compute the Integral Over Each Interval
We split the integral into two parts: from \(-4\) to \(0\) and from \(0\) to \(4\).

#### Part 1: Integral from \(-4\) to \(0\)
Here, \(|x| = -x\), so \(e^{|x|} = e^{-x}\). The integral becomes:
\[
\int_{-4}^0 e^{-x} \cdot \{x\} \, dx
\]
We break this into sub-intervals:
\[
\sum_{n=1}^4 \int_{-n}^{-n+1} e^{-x} (x + n) \, dx
\]
For each \(n\), compute:
\[
\int_{-n}^{-n+1} e^{-x} (x + n) \, dx
\]
Let \(u = x + n\), then \(du = dx\), and when \(x = -n\), \(u = 0\); when \(x = -n+1\), \(u = 1\). The integral becomes:
\[
\int_{0}^1 e^{-(u - n)} u \, du = e^{n} \int_{0}^1 e^{-u} u \, du
\]
The integral \(\int_{0}^1 e^{-u} u \, du\) can be computed using integration by parts:
\[
\int u e^{-u} \, du = -u e^{-u} - e^{-u} \Big|_{0}^1 = 1 - \frac{2}{e}
\]
Thus, the sum becomes:
\[
\sum_{n=1}^4 e^{n} \left(1 - \frac{2}{e}\right) = \left(1 - \frac{2}{e}\right) \sum_{n=1}^4 e^{n} = \left(1 - \frac{2}{e}\right) (e + e^2 + e^3 + e^4)
\]

#### Part 2: Integral from \(0\) to \(4\)
Here, \(|x| = x\), so \(e^{|x|} = e^{x}\). The integral becomes:
\[
\int_{0}^4 e^{x} \cdot \{x\} \, dx
\]
We break this into sub-intervals:
\[
\sum_{n=0}^3 \int_{n}^{n+1} e^{x} (x - n) \, dx
\]
For each \(n\), compute:
\[
\int_{n}^{n+1} e^{x} (x - n) \, dx
\]
Let \(u = x - n\), then \(du = dx\), and when \(x = n\), \(u = 0\); when \(x = n+1\), \(u = 1\). The integral becomes:
\[
\int_{0}^1 e^{u + n} u \, du = e^{n} \int_{0}^1 e^{u} u \, du
\]
The integral \(\int_{0}^1 e^{u} u \, du\) can be computed using integration by parts:
\[
\int u e^{u} \, du = u e^{u} - e^{u} \Big|_{0}^1 = 1
\]
Thus, the sum becomes:
\[
\sum_{n=0}^3 e^{n} \cdot 1 = \sum_{n=0}^3 e^{n} = 1 + e + e^2 + e^3
\]

### Step 4: Combine the Results
The total integral is the sum of Part 1 and Part 2:
\[
\left(1 - \frac{2}{e}\right) (e + e^2 + e^3 + e^4) + (1 + e + e^2 + e^3)
\]
Simplify:
\[
= (e + e^2 + e^3 + e^4) - \frac{2}{e}(e + e^2 + e^3 + e^4) + 1 + e + e^2 + e^3
\]
\[
= 1 + 2e + 2e^2 + 2e^3 + e^4 - 2(1 + e + e^2 + e^3)
\]
\[
= 1 + 2e + 2e^2 + 2e^3 + e^4 - 2 - 2e - 2e^2 - 2e^3
\]
\[
= -1 + e^4
\]

### Step 5: Numerical Approximation
Compute \(e^4 - 1\):
\[
e^4 \approx 54.5981500331
\]
\[
e^4 - 1 \approx 53.5981500331
\]

### Final Answer
\[
\boxed{e^4 - 1}
\]

The JSON output is:
```json
{"answer": "e^4 - 1", "numerical_answer": "53.5981500331"}
```