We wish to evaluate

  I = ∫₀² x^(1/2) (2 – x)^(–1/2) cos(√(x(2 – x))) dx.

Step 1. Change of variable

Let
  x = 2 sin²t  with  t ∈ [0, π/2].
Then
  dx = 4 sin t cos t dt,
  2 – x = 2 cos²t,
and
  √x = √(2) sin t,  √(2 – x) = √(2) cos t.
Thus,
  x^(1/2) (2 – x)^(–1/2) = (√(2) sin t)/(√(2) cos t) = tan t.
Also,
  √(x(2 – x)) = √(2 sin²t · 2 cos²t) = 2 sin t cos t.
Therefore, the cosine term becomes
  cos(√(x(2 – x))) = cos(2 sin t cos t).
But note that 2 sin t cos t = sin 2t so that
  cos(2 sin t cos t) = cos(sin 2t).

Step 2. Rewrite the integral in t–variable

Substituting everything in,
  I = ∫₀^(π/2) [tan t · cos(sin 2t) · (4 sin t cos t dt)].
Since tan t = sin t/cos t, we have
  tan t · (4 sin t cos t) = 4 sin²t.
Thus,
  I = 4 ∫₀^(π/2) sin²t · cos(sin 2t) dt.

Step 3. Substitute u = 2t

Let u = 2t so that du = 2 dt → dt = du/2.
When t = 0, u = 0; when t = π/2, u = π.
Also, sin²t = sin²(u/2). Hence the integral becomes
  I = 4 ∫₀^π sin²(u/2) cos(sin u) · (du/2)
     = 2 ∫₀^π sin²(u/2) cos(sin u) du.
Now use the double-angle formula for sine:
  sin²(u/2) = (1 – cos u)/2.
Thus,
  I = 2 ∫₀^π (1 – cos u)/2 · cos(sin u) du
     = ∫₀^π (1 – cos u) cos(sin u) du.
This splits into two integrals:
  I = ∫₀^π cos(sin u) du – ∫₀^π cos u cos(sin u) du.
Call these
  J₁ = ∫₀^π cos(sin u) du  and  J₂ = ∫₀^π cos u cos(sin u) du.

Step 4. Evaluate J₁ and J₂

A known integral formula (see, e.g., standard references on Bessel functions) is
  ∫₀^π cos(z sin u) du = π J₀(z)
with z a constant. Taking z = 1 gives
  J₁ = ∫₀^π cos(sin u) du = π J₀(1).

Now consider J₂. Write
  J₂ = ∫₀^π cos u cos(sin u) du.
Observe that if we express cos(sin u) as the real part of exp(i sin u), then one may write
  J₂ = Re{∫₀^π cos u e^(i sin u) du}.
Now notice that
  d/du (sin u) = cos u.
This suggests the substitution v = sin u. However, as u runs from 0 to π, the function sin u first increases (0 to 1, u: 0 → π/2) and then decreases (1 to 0, u: π/2 → π). Splitting the interval and changing variables in each piece shows that the two contributions cancel. (Alternatively, one may verify by symmetry that the integrand cos u cos(sin u) is antisymmetric about u = π/2.) Hence,
  J₂ = 0.

Thus,
  I = J₁ – J₂ = π J₀(1).

Step 5. Final answer

The exact answer is I = π J₀(1).

Step 6. Numerical evaluation

The Bessel function J₀(1) is approximately 0.7651976866. Therefore,
  I ≈ π × 0.7651976866 ≈ 3.1415926536 × 0.7651976866 ≈ 2.4041138066.

Thus, the final answers are:

Exact Answer: πJ₀(1)
Numerical Answer: 2.4041138066

{"answer": "\\pi J_0(1)", "numerical_answer": "2.4041138066"}