Let's compute the integral:
\[
I = \int_0^1 \frac{1}{x} \arccos x \, I_1(2x) \, dx
\]
where \( I_1 \) is the modified Bessel function of the first kind.

---

### Step 1: Series Expansion for \( I_1(2x) \)

Recall:
\[
I_1(2x) = \sum_{k=0}^\infty \frac{(x)^{2k+1}}{k! (k+1)!}
\]

So,
\[
I = \int_0^1 \frac{1}{x} \arccos x \left( \sum_{k=0}^\infty \frac{(2x)^{2k+1}}{k! (k+1)!} \right) dx
= \sum_{k=0}^\infty \frac{2^{2k+1}}{k! (k+1)!} \int_0^1 x^{2k} \arccos x \, dx
\]

---

### Step 2: Compute the Inner Integral

Let
\[
J_k = \int_0^1 x^{2k} \arccos x \, dx
\]

Let \( x = \cos \theta \), \( dx = -\sin \theta d\theta \), as \( x \) goes from 0 to 1, \( \theta \) goes from \( \pi/2 \) to 0.

So,
\[
J_k = \int_{x=0}^{x=1} x^{2k} \arccos x \, dx
= \int_{\theta=\pi/2}^{\theta=0} (\cos \theta)^{2k} \theta \cdot (-\sin \theta) d\theta
= \int_0^{\pi/2} (\cos \theta)^{2k} \theta \sin \theta d\theta
\]

---

### Step 3: Integration by Parts

Let \( u = \theta \), \( dv = (\cos \theta)^{2k} \sin \theta d\theta \).

Let \( v = -\frac{1}{2k+1} (\cos \theta)^{2k+1} \), since
\[
d((\cos \theta)^{2k+1}) = (2k+1) (\cos \theta)^{2k} (-\sin \theta) d\theta
\implies (\cos \theta)^{2k} \sin \theta d\theta = -\frac{1}{2k+1} d((\cos \theta)^{2k+1})
\]

So,
\[
J_k = \int_0^{\pi/2} \theta (\cos \theta)^{2k} \sin \theta d\theta
\]
Let \( u = \theta \), \( dv = (\cos \theta)^{2k} \sin \theta d\theta \), so \( du = d\theta \), \( v = -\frac{1}{2k+1} (\cos \theta)^{2k+1} \):

\[
J_k = u v \Big|_0^{\pi/2} - \int_0^{\pi/2} v du
= \left[ -\frac{\theta}{2k+1} (\cos \theta)^{2k+1} \right]_0^{\pi/2} + \frac{1}{2k+1} \int_0^{\pi/2} (\cos \theta)^{2k+1} d\theta
\]

At \( \theta = 0 \), \( \cos 0 = 1 \), so term is \( -\frac{0}{2k+1} \cdot 1 = 0 \).

At \( \theta = \pi/2 \), \( \cos(\pi/2) = 0 \), so term is \( -\frac{\pi/2}{2k+1} \cdot 0 = 0 \).

So the boundary terms vanish, and we have:
\[
J_k = \frac{1}{2k+1} \int_0^{\pi/2} (\cos \theta)^{2k+1} d\theta
\]

---

### Step 4: Evaluate the Cosine Integral

Recall:
\[
\int_0^{\pi/2} (\cos \theta)^n d\theta = \frac{\sqrt{\pi} \, \Gamma\left(\frac{n+1}{2}\right)}{2 \, \Gamma\left(\frac{n}{2} + 1\right)}
\]

Set \( n = 2k+1 \):

\[
\int_0^{\pi/2} (\cos \theta)^{2k+1} d\theta = \frac{\sqrt{\pi} \, \Gamma(k+1)}{2 \, \Gamma\left(k + \frac{3}{2}\right)}
\]

So,
\[
J_k = \frac{1}{2k+1} \cdot \frac{\sqrt{\pi} \, \Gamma(k+1)}{2 \, \Gamma\left(k + \frac{3}{2}\right)}
\]

---

### Step 5: Substitute Back

Recall:
\[
I = \sum_{k=0}^\infty \frac{2^{2k+1}}{k! (k+1)!} J_k
\]
So,
\[
I = \sum_{k=0}^\infty \frac{2^{2k+1}}{k! (k+1)!} \cdot \frac{1}{2k+1} \cdot \frac{\sqrt{\pi} \, \Gamma(k+1)}{2 \, \Gamma\left(k + \frac{3}{2}\right)}
\]
\[
= \sum_{k=0}^\infty \frac{2^{2k+1} \sqrt{\pi} \, \Gamma(k+1)}{k! (k+1)! (2k+1) 2 \Gamma\left(k + \frac{3}{2}\right)}
\]
\[
= \sum_{k=0}^\infty \frac{2^{2k} \sqrt{\pi} \, \Gamma(k+1)}{k! (k+1)! (2k+1) \Gamma\left(k + \frac{3}{2}\right)}
\]

But \( \Gamma(k+1) = k! \), so
\[
I = \sum_{k=0}^\infty \frac{2^{2k} \sqrt{\pi}}{(k+1)! (2k+1) \Gamma\left(k + \frac{3}{2}\right)}
\]

---

### Step 6: Closed Form

Let us check if this sum can be further simplified.

Alternatively, let's check if the original integral can be expressed in terms of known constants.

#### Alternative Approach: Integral Representation

Let us try to swap the order of integration and summation, as above, and see if the sum can be evaluated.

Alternatively, let's check for a closed form in terms of known constants.

#### Direct Evaluation

Let us try to compute the value numerically.

---

### Step 7: Numerical Evaluation

Let us compute the first few terms of the sum:

For \( k = 0 \):

- \( 2^{2k} = 1 \)
- \( (k+1)! = 1! = 1 \)
- \( 2k+1 = 1 \)
- \( \Gamma(k + 3/2) = \Gamma(3/2) = \frac{\sqrt{\pi}}{2} \)

So,
\[
\text{Term}_0 = \frac{1 \cdot \sqrt{\pi}}{1 \cdot 1 \cdot \frac{\sqrt{\pi}}{2}} = 2
\]

For \( k = 1 \):

- \( 2^{2k} = 4 \)
- \( (k+1)! = 2! = 2 \)
- \( 2k+1 = 3 \)
- \( \Gamma(1 + 3/2) = \Gamma(2.5) = \frac{3}{4} \sqrt{\pi} \)

So,
\[
\text{Term}_1 = \frac{4 \sqrt{\pi}}{2 \cdot 3 \cdot \frac{3}{4} \sqrt{\pi}} = \frac{4}{2 \cdot 3 \cdot \frac{3}{4}} = \frac{4}{2 \cdot 3 \cdot 0.75} = \frac{4}{4.5} = 0.\overline{8}
\]

For \( k = 2 \):

- \( 2^{4} = 16 \)
- \( (2+1)! = 6 \)
- \( 2k+1 = 5 \)
- \( \Gamma(2 + 3/2) = \Gamma(3.5) = \frac{3 \cdot 5}{8} \sqrt{\pi} = \frac{15}{8} \sqrt{\pi} \)

So,
\[
\text{Term}_2 = \frac{16 \sqrt{\pi}}{6 \cdot 5 \cdot \frac{15}{8} \sqrt{\pi}} = \frac{16}{6 \cdot 5 \cdot \frac{15}{8}} = \frac{16}{6 \cdot 5 \cdot 1.875} = \frac{16}{56.25} \approx 0.2844444444
\]

For \( k = 3 \):

- \( 2^{6} = 64 \)
- \( (3+1)! = 24 \)
- \( 2k+1 = 7 \)
- \( \Gamma(3 + 3/2) = \Gamma(4.5) = \frac{3 \cdot 5 \cdot 7}{16} \sqrt{\pi} = \frac{105}{16} \sqrt{\pi} \)

So,
\[
\text{Term}_3 = \frac{64 \sqrt{\pi}}{24 \cdot 7 \cdot \frac{105}{16} \sqrt{\pi}} = \frac{64}{24 \cdot 7 \cdot 6.5625} = \frac{64}{1102.5} \approx 0.0580381471
\]

Sum so far: \( 2 + 0.8888888889 + 0.2844444444 + 0.0580381471 = 3.2313714804 \)

For \( k = 4 \):

- \( 2^{8} = 256 \)
- \( (4+1)! = 120 \)
- \( 2k+1 = 9 \)
- \( \Gamma(4 + 3/2) = \Gamma(5.5) = \frac{3 \cdot 5 \cdot 7 \cdot 9}{32} \sqrt{\pi} = \frac{945}{32} \sqrt{\pi} \)

So,
\[
\text{Term}_4 = \frac{256 \sqrt{\pi}}{120 \cdot 9 \cdot \frac{945}{32} \sqrt{\pi}} = \frac{256}{120 \cdot 9 \cdot 29.53125} = \frac{256}{31839} \approx 0.0080439646
\]

Sum so far: \( 3.2394154450 \)

For \( k = 5 \):

- \( 2^{10} = 1024 \)
- \( (5+1)! = 720 \)
- \( 2k+1 = 11 \)
- \( \Gamma(5 + 3/2) = \Gamma(6.5) = \frac{3 \cdot 5 \cdot 7 \cdot 9 \cdot 11}{64} \sqrt{\pi} = \frac{10395}{64} \sqrt{\pi} \)

So,
\[
\text{Term}_5 = \frac{1024}{720 \cdot 11 \cdot 162.421875} = \frac{1024}{1286784} \approx 0.0007962362
\]

Sum so far: \( 3.2402116812 \)

For \( k = 6 \):

- \( 2^{12} = 4096 \)
- \( (6+1)! = 5040 \)
- \( 2k+1 = 13 \)
- \( \Gamma(6 + 3/2) = \Gamma(7.5) = \frac{3 \cdot 5 \cdot 7 \cdot 9 \cdot 11 \cdot 13}{128} \sqrt{\pi} = \frac{135135}{128} \sqrt{\pi} \)

So,
\[
\text{Term}_6 = \frac{4096}{5040 \cdot 13 \cdot 1056.5234375} = \frac{4096}{69127200} \approx 0.0000592632
\]

Sum so far: \( 3.2402709444 \)

For \( k = 7 \):

- \( 2^{14} = 16384 \)
- \( (7+1)! = 40320 \)
- \( 2k+1 = 15 \)
- \( \Gamma(7 + 3/2) = \Gamma(8.5) = \frac{3 \cdot 5 \cdot 7 \cdot 9 \cdot 11 \cdot 13 \cdot 15}{256} \sqrt{\pi} = \frac{2027025}{256} \sqrt{\pi} \)

So,
\[
\text{Term}_7 = \frac{16384}{40320 \cdot 15 \cdot 7925.09765625} = \frac{16384}{4790649600} \approx 0.0000034202
\]

Sum so far: \( 3.2402743646 \)

The terms are rapidly decreasing. So, the sum converges to about \( 3.2402743646 \).

---

### Step 8: Final Answer

#### Exact Answer

\[
I = \sum_{k=0}^\infty \frac{2^{2k} \sqrt{\pi}}{(k+1)! (2k+1) \Gamma\left(k + \frac{3}{2}\right)}
\]

#### Numerical Value

\[
I \approx 3.2402743646
\]

---

### Step 9: JSON Output

```json
{"answer": "\\sum_{k=0}^\\infty \\frac{2^{2k} \\sqrt{\\pi}}{(k+1)! (2k+1) \\Gamma\\left(k + \\frac{3}{2}\\right)}", "numerical_answer": "3.2402743646"}
```