We will show that the integral

  I = ∫₀² x^(–1/4) (2–x)^(–3/4) cos(√(x(2–x))) dx

may be written in closed‐form. One acceptable answer is

  I = π√2 · J₀(2),

where J₀(2) is the Bessel function of order 0 evaluated at 2. In what follows we describe one route for arriving at this answer.

──────────────────────────────
Step 1. Make the Substitution x = 2u

Define
  u = x/2  ⟹  x = 2u,  dx = 2 du.
Then the integration limits become u = 0 when x = 0 and u = 1 when x = 2. Also note that
  x^(–1/4) = (2u)^(–1/4) = 2^(–1/4) u^(–1/4)
  (2–x)^(–3/4) = [2(1–u)]^(–3/4) = 2^(–3/4) (1–u)^(–3/4).
Thus
  x^(–1/4)(2–x)^(–3/4) = 2^(–1/4–3/4) u^(–1/4) (1–u)^(–3/4) = 2^(–1) u^(–1/4) (1–u)^(–3/4).
Also, we have
  √(x(2–x)) = √(2u · 2(1–u)) = 2√(u(1–u)).
So the cosine factor becomes
  cos(√(x(2–x))) = cos(2√(u(1–u))).
Finally, with dx = 2 du the integral becomes
  I = ∫₀¹ u^(–1/4)(1–u)^(–3/4) cos(2√(u(1–u))) du.
(Notice that the factor 2 from dx cancels with the 2^(–1) from the algebra.)

──────────────────────────────
Step 2. Transform to a Standard Form

The integral now is
  I = ∫₀¹ u^(–1/4)(1–u)^(–3/4) cos(2√(u(1–u))) du.
This is of the form
  ∫₀¹ u^(μ–1)(1–u)^(ν–1) cos(2c√(u(1–u))) du,
with
  μ – 1 = –1/4 ⟹ μ = 3/4,
  ν – 1 = –3/4 ⟹ ν = 1/4,
  and c = 1.

There is a known formula (which you can verify by checking the limit c = 0)
  ∫₀¹ u^(μ–1)(1–u)^(ν–1) cos(2c√(u(1–u))) du = B(μ,ν) · {}₀F₁(; μ+ν; –c²),
where B(μ,ν) is the Beta–function.

In our case μ + ν = 3/4 + 1/4 = 1 so that
  B(3/4, 1/4) = Γ(3/4) Γ(1/4) / Γ(1) = Γ(3/4) Γ(1/4).
Also,
  {}₀F₁(; 1; –1).
There is a standard relation (see, e.g., in connection with Bessel functions)
  {}₀F₁(;1; –z²/4) = J₀(z).
Taking z = 2 we have
  {}₀F₁(;1; –1) = J₀(2).

Thus the integral becomes
  I = Γ(3/4) Γ(1/4) · J₀(2).

But an old classical result is
  Γ(1/4) Γ(3/4) = π√2.
Thus we obtain the compact result
  I = π√2 · J₀(2).

──────────────────────────────
Step 3. Numerical Evaluation

A standard numerical value is:
  J₀(2) ≈ 0.2238907791,
and
  π√2 ≈ 4.4428829382.
Thus,
  I ≈ 4.4428829382 × 0.2238907791 ≈ 0.9947142500.

──────────────────────────────
Final Answer

We thus have shown that

  I = π√2 · J₀(2)     (with I ≈ 0.9947142500).

As required, we now output the answer in the prescribed JSON format.

{"answer": "$\\pi\\sqrt{2}\\,J_0(2)$", "numerical_answer": "0.9947142500"}