Let's solve the definite integral:
\[
I = \int_0^2 x \arcsin\left(0.5 \sqrt{x(2-x)}\right)\, dx
\]

### Step 1: Substitution

Let us start by substituting:
\[
x = 1 - \cos\theta
\]
for \(\theta \in [0, \pi]\), since when \(x=0\), \(\theta=0\), and when \(x=2\), \(\theta=\pi\).

Compute \(dx\):
\[
dx = \sin\theta\, d\theta
\]

Compute \(x(2-x)\):

\[
x(2-x) = (1-\cos\theta)[2-(1-\cos\theta)] = (1-\cos\theta)(1+\cos\theta) = 1 - \cos^2\theta = \sin^2\theta
\]
So,
\[
\sqrt{x(2-x)} = \sin\theta
\]
Therefore,
\[
0.5 \sqrt{x(2-x)} = 0.5 \sin\theta
\]

So,
\[
I = \int_{\theta=0}^{\pi} (1 - \cos\theta) \arcsin\left(0.5\sin\theta\right) \sin\theta\, d\theta
\]

Expanding:
\[
I = \int_0^\pi \left[ \sin\theta\, \arcsin\left(0.5\sin\theta\right)
        - \sin\theta \cos\theta\, \arcsin\left(0.5\sin\theta\right) \right] d\theta
\]
Or,
\[
I = I_1 - I_2
\]
where
\[
I_1 = \int_0^\pi \sin\theta\, \arcsin\left(0.5\sin\theta\right) d\theta
\]
\[
I_2 = \int_0^\pi \sin\theta \cos\theta\, \arcsin\left(0.5\sin\theta\right) d\theta
\]

---

### Step 2: Evaluate \( I_1 \) and \( I_2 \)

#### For \( I_1 \):

Let’s use the substitution \( t = \sin\theta \), so when \(\theta=0\), \(t=0\); when \(\theta=\pi\), \(t=0\). The range of \(\sin\theta\) over \(0\) to \(\pi\) is 0 to 1 and back to 0; so we can write:
\[
I_1 = \int_0^\pi \sin\theta\, \arcsin\left(0.5\sin\theta\right) d\theta
\]
This is symmetric about \(\theta = \frac{\pi}{2}\), considering the function.

But evaluating directly may not simplify further analytically; instead, let's look for an alternative approach.

#### Let’s Try Another Substitution

Let’s go back to the original integral:
\[
J = \int_0^2 x \arcsin\left(0.5\sqrt{x(2-x)}\right)\, dx
\]
Let’s use
\[
x = 1 - \cos\theta, \quad dx = \sin\theta\, d\theta, \quad x(2-x) = \sin^2\theta
\]
as above.

So, re-expressing the integral:
\[
I = \int_0^\pi (1 - \cos\theta) \arcsin\left( \frac{1}{2} \sin\theta \right) \sin\theta\, d\theta
\]
\[
= \int_0^\pi \sin\theta\, \arcsin\left( \frac{1}{2} \sin\theta \right) d\theta - \int_0^\pi \sin\theta \cos\theta\, \arcsin\left( \frac{1}{2} \sin\theta \right) d\theta
\]

Let’s focus on performing integration by parts on \(I_1\):

Let’s try to compute:
\[
I_1 = \int_0^\pi \sin\theta\, \arcsin\left(\frac{1}{2} \sin\theta \right) d\theta
\]

Let:
\[
u = \arcsin\left(\frac{1}{2} \sin\theta\right), \quad dv = \sin\theta\, d\theta
\]
Then,
\[
du = \frac{1}{\sqrt{1 - (\frac{1}{2}\sin\theta)^2}} \cdot \frac{1}{2}\cos\theta\, d\theta
= \frac{\cos\theta}{2\sqrt{1 - \frac{1}{4} \sin^2\theta}}\, d\theta
\]
\[
v = -\cos\theta
\]

So,
\[
I_1 = uv \Big|_0^\pi - \int_0^\pi v\, du
\]
\[
= \left[ -\cos\theta \cdot \arcsin\left( \frac{1}{2} \sin\theta \right) \right]_0^\pi
+ \int_0^\pi \cos\theta \cdot \frac{\cos\theta}{2\sqrt{1-\frac{1}{4}\sin^2\theta}} d\theta
\]

\[
= \left[ -\cos\theta \cdot \arcsin\left( \frac{1}{2} \sin\theta \right) \right]_0^\pi
+ \frac{1}{2} \int_0^\pi \frac{\cos^2\theta}{\sqrt{1-\frac{1}{4}\sin^2\theta}} d\theta
\]

Let's compute the boundary term:

- At \(\theta = 0\), \(\cos\theta = 1\), \(\sin\theta = 0\), so \(\arcsin(0) = 0\), term is 0.
- At \(\theta = \pi\), \(\cos\theta = -1\), \(\sin\theta = 0\), \(\arcsin(0) = 0\), term is also 0.

So the boundary term is zero.

Thus,
\[
I_1 = \frac{1}{2} \int_0^\pi \frac{\cos^2\theta}{\sqrt{1-\frac{1}{4}\sin^2\theta}} d\theta
\]

Now, recall:
\[
I_2 = \int_0^\pi \sin\theta\cos\theta\, \arcsin\left(\frac{1}{2}\sin\theta\right) d\theta
\]

Let’s set
\[
w = \arcsin(0.5\sin\theta)
\]
Let’s try integration by parts with
\[
u = \arcsin(0.5\sin\theta), \quad dv = \sin\theta\cos\theta\, d\theta
\]
Then,
\[
du = \frac{\cos\theta}{2\sqrt{1 - (0.25)\sin^2\theta}} d\theta
\]
\[
v = \int \sin\theta\cos\theta d\theta = \frac{1}{2}\int \sin(2\theta)d\theta 
= -\frac{1}{4} \cos(2\theta)
\]

Then:
\[
I_2 = uv \Big|_0^\pi - \int_0^\pi v\, du
\]
But at \(\theta = 0\), \(\arcsin(0)=0\), at \(\theta=\pi\), \(\arcsin(0)=0\), and \(\cos(2\cdot 0) = \cos(0) = 1\), \(\cos(2\pi) = 1\), so boundary term is zero.

Therefore,
\[
I_2 = - \int_0^\pi \left(-\frac{1}{4} \cos(2\theta) \cdot \frac{\cos\theta}{2\sqrt{1-\frac{1}{4}\sin^2\theta}} \right) d\theta
\]
\[
= \frac{1}{8} \int_0^\pi \cos(2\theta)\cos\theta \frac{1}{\sqrt{1 - \frac{1}{4}\sin^2\theta}} d\theta
\]

Recall that
\[
\cos(2\theta)\cos\theta = \frac{1}{2}\left[\cos(\theta)+\cos(3\theta)\right]
\]

So,

\[
I_2 = \frac{1}{8} \int_0^\pi \left[ \cos\theta + \cos(3\theta) \right] \frac{1}{\sqrt{1 - \frac{1}{4}\sin^2\theta}} d\theta
\]

Splitting,
\[
I_2 = \frac{1}{8} \int_0^\pi \cos\theta \frac{d\theta}{\sqrt{1 - \frac{1}{4}\sin^2\theta}}
+ \frac{1}{8} \int_0^\pi \cos(3\theta) \frac{d\theta}{\sqrt{1 - \frac{1}{4}\sin^2\theta}}
\]

Therefore, our integral is:
\[
I = I_1 - I_2 =
\frac{1}{2} \int_0^\pi \frac{\cos^2\theta}{\sqrt{1 - \frac{1}{4}\sin^2\theta}} d\theta
- \frac{1}{8} \int_0^\pi \cos\theta \frac{d\theta}{\sqrt{1 - \frac{1}{4}\sin^2\theta}}
- \frac{1}{8} \int_0^\pi \cos(3\theta) \frac{d\theta}{\sqrt{1 - \frac{1}{4}\sin^2\theta}}
\]

Let's combine the terms:

Note that
\[
\cos^2\theta = \frac{1 + \cos(2\theta)}{2}
\]
So:
\[
\frac{1}{2} \int_0^\pi \frac{\cos^2\theta}{\sqrt{1 - \frac{1}{4}\sin^2\theta}} d\theta
= \frac{1}{4} \int_0^\pi \frac{d\theta}{\sqrt{1 - \frac{1}{4}\sin^2\theta}}
+ \frac{1}{4} \int_0^\pi \frac{\cos(2\theta) d\theta}{\sqrt{1 - \frac{1}{4}\sin^2\theta}}
\]

Now assemble:
\[
I = 
\frac{1}{4} \int_0^\pi \frac{d\theta}{\sqrt{1 - \frac{1}{4}\sin^2\theta}}
+ \frac{1}{4} \int_0^\pi \frac{\cos(2\theta)\, d\theta}{\sqrt{1 - \frac{1}{4}\sin^2\theta}}
- \frac{1}{8} \int_0^\pi \frac{\cos\theta\, d\theta}{\sqrt{1 - \frac{1}{4}\sin^2\theta}}
- \frac{1}{8} \int_0^\pi \frac{\cos(3\theta)\, d\theta}{\sqrt{1 - \frac{1}{4}\sin^2\theta}}
\]

Or grouping:
\[
I = 
\frac{1}{4} K(k)
+ \frac{1}{4} C_2
- \frac{1}{8} C_1
- \frac{1}{8} C_3
\]
where \( K(k) = \int_0^\pi \frac{d\theta}{\sqrt{1-k^2 \sin^2\theta}} \) is the complete elliptic integral of the first kind with \( k^2 = 1/4 \), i.e., \( k = 1/2 \), and \(C_n = \int_0^\pi \frac{\cos (n\theta) d\theta}{\sqrt{1-\frac{1}{4}\sin^2\theta}} \).

Now, standard integrals yield:
\[
\int_0^\pi \frac{\cos(n\theta)\, d\theta}{\sqrt{1 - k^2 \sin^2\theta}} = \pi P_{n}(k)
\]
for certain functions \(P_n(k)\), but let's check the known values.

But let's write the answer in terms of complete elliptic integrals for the first kind \(K(k)\) and second kind \(E(k)\):

Recall (see Gradshteyn & Ryzhik 3.677):

\[
\int_0^\pi \frac{d\theta}{\sqrt{1 - k^2 \sin^2 \theta}} = 2 K(k)
\]
But the usual definition is over \(0\) to \(\pi/2\). Since the integrand is even about \(\pi/2\),
\[
\int_0^\pi \frac{d\theta}{\sqrt{1 - k^2 \sin^2 \theta}} = 2 K(k)
\]

But let's use the version from 0 to \(\pi/2\). That is,
\[
\int_0^\pi f(\theta) \, d\theta = 2\int_0^{\pi/2} f(\theta) d\theta \text{ if } f(\pi - \theta) = f(\theta).
\]

Since all of our terms are even or can be written over \(0\) to \(\pi/2\):

So,
\[
K\left(\frac{1}{2}\right) = \int_0^{\pi/2} \frac{d\theta}{\sqrt{1 - \frac{1}{4} \sin^2\theta}}
\]
Thus,
\[
\int_0^\pi \frac{d\theta}{\sqrt{1 - \frac{1}{4} \sin^2\theta}} = 2 K\left(\frac{1}{2}\right)
\]
Similarly, for even multiples of \(\theta\), the integral is non-zero, for odd multiples (like \(\cos\theta\)), the integral may vanish by symmetry.

Let’s compute \(C_1, C_2, C_3\):

Let’s check \(C_1\):

\[
C_1 = \int_0^\pi \frac{\cos\theta\, d\theta}{\sqrt{1-\frac{1}{4}\sin^2\theta}}
\]
But the integrand is odd in \(\theta\) about \(\pi/2\), so integrates to zero over \(0\) to \(\pi\). Therefore,
\[
C_1 = 0
\]

Similarly, \(C_3\) (since \(\cos(3\theta)\)) also integrates to zero over \(0\) to \(\pi\).

\(C_2\) is:

\[
C_2 = \int_0^\pi \frac{\cos (2\theta)\, d\theta}{\sqrt{1-\frac{1}{4}\sin^2\theta}}
\]

Now, this is non-zero.

From Gradshteyn & Ryzhik 3.674.3:
\[
\int_0^\pi \frac{\cos (2n\theta) d\theta}{\sqrt{1 - k^2 \sin^2\theta}} = \frac{2\pi}{\pi} Q_{n-1}(k)
\]
But more useful is to try and write this in terms of complete elliptic integrals.

But, from Byrd & Friedman, or computation tables (or via the double angle formula), we can write:
\[
\int_0^\pi \frac{\cos (2\theta)\, d\theta}{\sqrt{1 - k^2\sin^2\theta}} = 2 \int_0^{\pi/2} \frac{\cos (2\theta)\, d\theta}{\sqrt{1 - k^2\sin^2\theta}}
\]
And this is (see Gradshteyn & Ryzhik 3.677.4):
\[
\int_0^{\pi/2} \frac{\cos(2\theta)\, d\theta}{\sqrt{1-k^2\sin^2\theta}} = \frac{1}{k^2}\left[(1 - k^2) K(k) - E(k)\right]
\]
So over \(0\) to \(\pi\):
\[
\int_0^\pi \frac{\cos(2\theta)\, d\theta}{\sqrt{1-k^2\sin^2\theta}} = 2 \times \frac{1}{k^2}\left[(1 - k^2) K(k) - E(k)\right]
\]

Let's put all this together:

Therefore,
\[
I = 
\frac{1}{4} \times 2 K(k) + \frac{1}{4} \times 2 \frac{(1-k^2) K(k) - E(k)}{k^2}
\]
where \(k = \frac{1}{2}\).

Thus,

\[
I = \frac{1}{2} K\left(\frac{1}{2}\right) + \frac{1}{2} \frac{(1 - (1/4)) K(1/2) - E(1/2)}{1/4}
= \frac{1}{2} K\left(\frac{1}{2}\right) + 2 \left((1 - \frac{1}{4}) K(1/2) - E(1/2)\right)
\]
\[
= \frac{1}{2} K\left(\frac{1}{2}\right) + 2 \cdot \left( \frac{3}{4} K(1/2) - E(1/2)\right)
\]
\[
= \frac{1}{2} K\left(\frac{1}{2}\right) + \frac{3}{2} K\left(\frac{1}{2}\right) - 2 E\left(\frac{1}{2}\right)
\]
\[
= 2 K\left(\frac{1}{2}\right) - 2 E\left(\frac{1}{2}\right)
\]
\[
= 2 \left[ K\left(\frac{1}{2}\right) - E\left(\frac{1}{2}\right) \right]
\]

**Thus:**
\[
\boxed{
I = 2 \left[ K\left(\frac{1}{2}\right) - E\left(\frac{1}{2}\right) \right]
}
\]

Where \(K(k)\) and \(E(k)\) are the complete elliptic integrals of the first and second kind, respectively.

---

### Step 3: Numerical Approximation

Let’s compute \(K(1/2)\) and \(E(1/2)\):

Using standard values:

- \( K(1/2) \approx 1.6857503548 \)
- \( E(1/2) \approx 1.4674622093 \)

So:
\[
I \approx 2 \times (1.6857503548 - 1.4674622093)
= 2 \times 0.2182881455
= 0.4365762910
\]

---

### Step 4: Final Answer in JSON

```json
{"answer": "2 \\left[ K\\left(\\tfrac{1}{2}\\right) - E\\left(\\tfrac{1}{2}\\right) \\right]", "numerical_answer": "0.4365762910"}
```