<think>
Okay, let's tackle this integral: the definite integral from 0 to 2 of x times H₃(√(x(2−x))) dx. Hmm, H₃ is the third Hermite polynomial. First, I need to recall what the Hermite polynomials are. Hermite polynomials are a set of orthogonal polynomials that arise in probability, such as in the definition of the Hermite functions. The third Hermite polynomial, H₃(y), if I remember correctly, is given by H₃(y) = 8y³ - 12y. Let me confirm that. Yes, the general formula for Hₙ(y) is (-1)^n e^{y²} dⁿ/dyⁿ e^{-y²}, so for n=3, calculating that derivative would give H₃(y) = 8y³ - 12y. So that's correct.

So substituting the argument √(x(2−x)) into H₃, we have H₃(√(x(2−x))) = 8[√(x(2−x))]³ - 12√(x(2−x)). Therefore, the integrand becomes x*(8[x(2−x)]^(3/2) - 12[x(2−x)]^(1/2)). Let me write that out:

Integral from 0 to 2 of [8x(x(2−x))^(3/2) - 12x(x(2−x))^(1/2)] dx.

So, let's split this into two separate integrals:

8∫₀² x(x(2−x))^(3/2) dx - 12∫₀² x(x(2−x))^(1/2) dx.

Hmm, these integrals look a bit complicated, but maybe a substitution can help. The expression under the square root is x(2−x), which is symmetric around x=1. Let me consider a substitution to simplify this. Let’s set t = x - 1, which would shift the interval to be from -1 to 1. But maybe another substitution. Alternatively, since the limits are from 0 to 2, and the function x(2−x) is symmetric around x=1, perhaps substituting u = x - 1, so that the integral becomes symmetric. Let me try that.

Let u = x - 1. Then x = u + 1, and when x=0, u=-1; x=2, u=1. The differential dx = du. Then, x(2−x) = (u+1)(2 - (u+1)) = (u+1)(1 - u) = 1 - u². So, x(2−x) = 1 - u². Therefore, √(x(2−x)) = √(1 - u²). So, the integrand becomes:

For the first integral: 8*(u + 1)*(1 - u²)^(3/2) du, integrated from u=-1 to u=1.

Similarly, the second integral: -12*(u + 1)*(1 - u²)^(1/2) du, integrated from u=-1 to u=1.

So, combining both terms, the integral becomes:

8∫_{-1}^1 (u + 1)(1 - u²)^(3/2) du - 12∫_{-1}^1 (u + 1)(1 - u²)^(1/2) du.

Now, let's split each integral into two parts. For example, the first integral is 8[∫_{-1}^1 u(1 - u²)^(3/2) du + ∫_{-1}^1 (1 - u²)^(3/2) du]. Similarly for the second integral: -12[∫_{-1}^1 u(1 - u²)^(1/2) du + ∫_{-1}^1 (1 - u²)^(1/2) du].

Now, notice that the integrals of odd functions over symmetric intervals. The term with u*(1 - u²)^{k} is an odd function because u is replaced by -u, and the function becomes -u*(1 - (-u)^2)^k = -u*(1 - u²)^k, which is the negative of the original. Therefore, the integrals of the odd functions over [-1,1] will be zero. So, the integrals involving u*(1 - those will vanish. Therefore, the first integral reduces to 8*∫_{-1}^1 (1 - u²)^(3/2) du, and the second integral reduces to -12*∫_{-1}^1 (1 - u²)^(1/2) du.

So, now we have:

8 * 2∫₀}^1 (1 - u²)^(3/2) du - 12 * 2∫₀}^1 (1 - u²)^(1/2) du.

Because the function (1 - u²)^k is even, so integrating from -1 to 1 is twice the integral from 0 to 1.

Therefore, simplifying:

16∫₀^1 (1 - u²)^(3/2) du - 24∫₀^1 (1 - u²)^(1/2) du.

Now, these integrals are standard Beta function integrals. Recall that ∫₀^1 (1 - u²)^k du can be expressed in terms of the Beta function. Let me recall that ∫₀^1 u^{m}(1 - u²)^n du = (1/2) B((m+1)/2, n +1) ), where B is the Beta function. Alternatively, using substitution t = u², but let's see.

Alternatively, let’s use substitution u = sinθ. For the first integral, ∫ (1 - u²)^(3/2) du. Let u = sinθ, then du = cosθ dθ, and when u=0, θ=0; u=1, θ=π/2. Then, (1 - u²)^(3/2) = cos^3θ. So the integral becomes ∫₀^{π/2} cos^3θ * cosθ dθ = ∫₀^{π/2} cos^4θ dθ.

Similarly, the second integral ∫₀^1 (1 - u²)^(1/2) du is ∫₀^{π/2} cos^2θ dθ.

So, let's compute these.

First integral: ∫₀^{π/2} cos^4θ dθ. The formula for ∫ cos^nθ dθ from 0 to π/2 is (sqrt(π)/2) * Γ((n+1)/2) / Γ((n+2)/2)). For n even, there's a formula. Alternatively, using reduction formulas. For n=4, we can use the identity cos^4θ = (3/8) + (1/2)cos2θ) + (1/8)cos4θ). Integrating term by term from 0 to π/2:

∫ cos^4θ dθ = (3/8)(π/2) + (1/2)(0) + (1/8)(0) = 3π/16.

Wait, let me check that. Alternatively, using the formula for even n: ∫₀^{π/2} cos^{2m}θ dθ = (π/2) * (2m-1)!! / (2m)!!). For m=2, that's (π/2)*(3!!)/(4!!) = (π/2)*(3*1)/(4*2) )= (π/2)*(3/8) = 3π/16. Yes, that's correct.

Similarly, for the second integral ∫₀^{π/2} cos^2θ dθ. Using the same formula, m=1: (π/2)*(1!!)/(2!!) = (π/2)*(1/2) = π/4.

Therefore, substituting back:

First integral (3π/16) * 16 (from the 16 in front) gives 16*(3π/16) = 3π.

Second integral: π/4 * 24 (but with a negative sign) gives -24*(π/4) = -6π.

Therefore, the total integral is 3π -6π = -3π.

Wait, that can't be right. Wait, let's check the coefficients again.

Wait, after substitution, the first integral was 16 * ∫₀^1 (1 - u²)^(3/2) du = 16*(3π/16) = 3π.

The second integral was -24 * ∫₀^1 (1 - u²)^(1/2) du = -24*(π/4) = -6π.

So total integral is 3π -6π = -3π. But wait, the original integrand was x*H3(...), and H3 is 8y³ -12y. Let me check if there's a mistake in the substitution steps.

Wait, but H3(√(x(2−x))) = 8(√(x(2−x)))^3 -12√(x(2−x)). Then, the integrand is x*(8(x(2−x))^{3/2} -12(x(2−x))^{1/2}).

Then, when we did substitution u = x -1, x = u +1, and x(2−x) =1 -u². So, (x(2−x))^{3/2} = (1 -u²)^{3/2}, and (x(2−x))^{1/2} = (1 -u²)^{1/2}. Then, the integrand becomes (u +1)*(8(1 -u²)^{3/2} -12(1 -u²)^{1/2}).

Then, expanding, we have 8(u +1)(1 -u²)^{3/2} -12(u +1)(1 -u²)^{1/2}. Then, splitting into integrals over u and 1, but the u terms are odd functions, so their integrals vanish. So we have 8*2∫₀^1 (1 -u²)^{3/2} du -12*2∫₀^1 (1 -u²)^{1/2} du. Wait, but 8*2 is 16, and -12*2 is -24. Then, integrating gives 16*(3π/16) -24*(π/4) = 3π -6π = -3π. So the result is -3π. But wait, integrating from 0 to 2, the integrand is x*H3(...). But H3 is a polynomial, but the argument is sqrt(x(2−x)), which is real between 0 and 2. However, the result is negative? Let me check if the substitution steps are correct.

Wait, but when we did the substitution u = x -1, the limits from x=0 to x=2 become u=-1 to u=1. Then, the integrand becomes (u +1) times the H3 term. But when we split the integral into u and 1 parts, the u terms integrate to zero. So the remaining terms are the integrals of 1*(1 -u²)^{3/2} and 1*(1 -u²)^{1/2}. Then, multiplied by 8 and -12 respectively, and then multiplied by 2 (from the symmetric interval). So, 8*2*∫₀^1 (1 -u²)^{3/2} du -12*2*∫₀^1 (1 -u²)^{1/2} du. Then, substituting the integrals as 3π/16 and π/4. Wait, 16*(3π/16) is 3π, and -24*(π/4) is -6π. So total is -3π. Hmm.

But let's check if the integral of x*H3(...) from 0 to 2 is indeed negative. Let me consider the function H3(y) =8y³ -12y. If y is between 0 and 1, since x is between 0 and 2, x(2−x) is between 0 and 1 (since x(2−x) is a downward parabola with maximum at x=1, where it's 1*1=1). So y = sqrt(x(2−x)) is between 0 and 1. So H3(y) =8y³ -12y. Let's see, for y in (0,1), 8y³ -12y = 4y(2y² -3). Since y is positive, the sign depends on 2y² -3. For y < sqrt(3/2) ≈1.2247, which is always true since y <=1, so 2y² -3 is negative. Therefore, H3(y) is negative in (0,1). So the integrand x*H3(y) is x times a negative number, so the integrand is negative over the entire interval. Therefore, the integral should be negative. So -3π is plausible.

But let me check with a numerical approximation. Let's compute the integral numerically to see if it's approximately -9.42477796... which is -3π (since π≈3.1415926535, 3π≈9.42477796077). So negative of that is -9.42477796077. Let me check with a numerical approximation.

Alternatively, let's compute the integral step by step. Let's take x from 0 to 2. Let's pick some sample points. For example, at x=0, the integrand is 0*H3(0) =0. At x=1, y= sqrt(1*1)=1, H3(1)=8*1 -12*1= -4, so integrand is 1*(-4)= -4. At x=2, integrand is 2*H3(0)=0. The function is negative in between. So the integral is the area under a curve that is negative from 0 to 2, so the result should be negative, which matches our analytical result of -3π.

Therefore, the exact answer is -3π, and the numerical approximation is approximately -9.42477796077.

But let me verify the steps again to make sure. Let's go back.

Original integral: ∫₀² x H₃(√(x(2−x))) dx.

H₃(y) =8y³ -12y.

So integrand: x*(8 [x(2−x)]^{3/2} -12 [x(2−x)]^{1/2}).

Substitution u = x -1, x = u +1, dx = du, limits from -1 to1.

x(2−x) = (u+1)(1 -u) =1 -u².

So integrand becomes (u +1)*(8(1 -u²)^{3/2} -12(1 -u²)^{1/2}).

Expanding: 8(u +1)(1 -u²)^{3/2} -12(u +1)(1 -u²)^{1/2}.

Split into two integrals: 8∫_{-1}^1 (u +1)(1 -u²)^{3/2} du -12∫_{-1}^1 (u +1)(1 -u²)^{1/2} du.

Each integral can be split into ∫ u*(...) du + ∫ (...) du. The integrals with u*(...) are odd functions, so they integrate to zero. Therefore, each integral reduces to ∫_{-1}^1 (...) du, which is 2∫₀^1 (...) du.

So first term: 8*2∫₀^1 (1 -u²)^{3/2} du =16∫₀^1 (1 -u²)^{3/2} du.

Second term: -12*2∫₀^1 (1 -u²)^{1/2} du = -24∫₀^1 (1 -u²)^{1/2} du.

Now, compute these integrals. As before, using substitution u = sinθ, then (1 -u²)^{1/2} = cosθ, du = cosθ dθ.

For ∫ (1 -u²)^{3/2} du from 0 to1:

u = sinθ, θ from 0 to π/2.

Integral becomes ∫ cos^3θ * cosθ dθ = ∫ cos^4θ dθ = 3π/16.

Similarly, ∫ (1 -u²)^{1/2} du from 0 to1 is ∫ cos^2θ dθ = π/4.

Therefore, substituting back:

16*(3π/16) =3π.

-24*(π/4) = -6π.

Total integral: 3π -6π = -3π.

Yes, that's correct. So the exact answer is -3π. The numerical approximation is -3*3.141592653589793 ≈ -9.42477796076938. Rounded to 10 decimal places, that's -9.4247779608.

But let me check with more precise calculation. π is approximately 3.1415926535897932384626433832795. So 3π is 9.4247779607693797153879301498385. Therefore, -3π is approximately -9.424777960769379715, which rounded to 10 decimal places is -9.4247779608.

Therefore, the final answer is {"answer": "-3\\pi", "numerical_answer": -9.4247779608}.
</think>

{"answer": "-3\\pi", "numerical_answer": -9.4247779608}