To solve the definite integral \(\int\limits_0^\infty x^{2-1}e^{-1.0x^2}H_2(1.0x)dx\), we need to understand the components involved. Here, \(H_2(x)\) is the Hermite polynomial of degree 2, which is given by:

\[ H_2(x) = 4x^2 - 2 \]

The integral can be rewritten as:

\[ \int\limits_0^\infty x^{1}e^{-x^2}(4x^2 - 2)dx \]

We can split this into two separate integrals:

\[ \int\limits_0^\infty x^{1}e^{-x^2}(4x^2)dx - \int\limits_0^\infty x^{1}e^{-x^2}(2)dx \]

Let's solve each integral separately.

### First Integral: \(\int\limits_0^\infty x^{1}e^{-x^2}(4x^2)dx\)

\[ 4 \int\limits_0^\infty x^{3}e^{-x^2}dx \]

To solve this, we use the substitution \(u = x^2\), hence \(du = 2x dx\) or \(dx = \frac{du}{2x}\). When \(x = 0\), \(u = 0\), and when \(x \to \infty\), \(u \to \infty\). The integral becomes:

\[ 4 \int\limits_0^\infty x^{3}e^{-x^2}dx = 4 \int\limits_0^\infty x^{3}e^{-u} \frac{du}{2x} = 2 \int\limits_0^\infty x^{2}e^{-u} du \]

Since \(x^2 = u\), we have:

\[ 2 \int\limits_0^\infty u e^{-u} du \]

This is a standard integral, and we know that:

\[ \int\limits_0^\infty u e^{-u} du = \Gamma(2) = 1! = 1 \]

So,

\[ 2 \int\limits_0^\infty u e^{-u} du = 2 \cdot 1 = 2 \]

### Second Integral: \(\int\limits_0^\infty x^{1}e^{-x^2}(2)dx\)

\[ 2 \int\limits_0^\infty x e^{-x^2}dx \]

Using the same substitution \(u = x^2\), \(du = 2x dx\), we get:

\[ 2 \int\limits_0^\infty x e^{-x^2}dx = 2 \int\limits_0^\infty e^{-u} \frac{du}{2} = \int\limits_0^\infty e^{-u} du \]

This is another standard integral:

\[ \int\limits_0^\infty e^{-u} du = 1 \]

So,

\[ 2 \int\limits_0^\infty x e^{-x^2}dx = 2 \cdot 1 = 2 \]

### Combining the Results

Combining the results of the two integrals, we get:

\[ 2 - 2 = 0 \]

### Numerical Approximation

Since the exact result is 0, the numerical approximation is also 0.

### Final Answer

The final answer in the requested JSON format is:

```json
{"answer": "0", "numerical_answer": "0.0000000000"}
```