<think>
Okay, let's see. I need to compute the definite integral of x times (log x) squared from 1 to e. Hmm, integration by parts might be the way to go here since we have a product of functions. The integrand is x*(ln x)^2. 

First, I remember that integration by parts formula is ∫u dv = uv - ∫v du. So I need to choose u and dv. Let me think, usually, we let u be the part that becomes simpler when differentiated. Here, (ln x)^2 is the part that might simplify when differentiated. But wait, the other part is x, which when integrated becomes (1/2)x². Maybe I should set u = (ln x)^2 and dv = x dx. Let's try that.

So, u = (ln x)^2. Then du/dx would be 2*(ln x)*(1/x) by the chain rule. So du = 2*(ln x)/x dx. And dv = x dx, so integrating dv gives v = (1/2)x².

Applying integration by parts: ∫x(ln x)^2 dx = uv - ∫v du. That would be (ln x)^2*(1/2)x² - ∫(1/2)x² * 2*(ln x)/x dx. Simplify the integral part: the 1/2 and 2 cancel out, and x²/x is x. So the integral becomes (1/2)x²(ln x)^2 - ∫x*(ln x) dx.

Now, we have another integral to solve: ∫x*(ln x) dx. Again, use integration by parts here. Let me set u = ln x this time, so du = 1/x dx. Then dv = x dx, so v = (1/2)x². Applying the formula: uv - ∫v du = (ln x)*(1/2)x² - ∫(1/2)x²*(1/x) dx. Simplify the integral: (1/2)x² ln x - (1/2)∫x dx. The integral of x dx is (1/2)x², so this becomes (1/2)x² ln x - (1/2)*(1/2)x² + C = (1/2)x² ln x - (1/4)x² + C.

Putting this back into the original integral: the original integral is (1/2)x²(ln x)^2 - [ (1/2)x² ln x - (1/4)x² ] evaluated from 1 to e. So combining terms, the antiderivative is (1/2)x²(ln x)^2 - (1/2)x² ln x + (1/4)x².

Now, evaluate this from 1 to e. Let's compute each term at e and 1.

First, at x = e:

Term 1: (1/2)e²*(ln e)^2. Since ln e = 1, so this is (1/2)e²*(1)^2 = (1/2)e².

Term 2: - (1/2)e²*(ln e) = - (1/2)e²*1 = - (1/2)e².

Term 3: + (1/4)e².

So adding these together: (1/2)e² - (1/2)e² + (1/4)e² = (1/4)e².

Now, evaluate at x = 1:

Term 1: (1/2)(1)^2*(ln 1)^2. ln 1 is 0, so this term is 0.

Term 2: - (1/2)(1)^2*(ln 1) = 0.

Term 3: + (1/4)(1)^2 = 1/4.

So the value at 1 is 0 - 0 + 1/4 = 1/4.

Subtracting the lower limit from the upper limit: (1/4)e² - 1/4 = (e² - 1)/4.

So the exact answer is (e² - 1)/4. Let me check that again. Wait, when I evaluated at e, the three terms added up to (1/4)e², and at 1, it's 1/4. So subtracting, (1/4)e² - 1/4 = (e² - 1)/4. That seems right.

Now, for the numerical approximation. e is approximately 2.718281828459045. So e squared is e*e ≈ 7.389056098930649. Then e² -1 ≈ 6.389056098930649. Divide by 4: 6.389056098930649 /4 ≈ 1.5972640247326623. Rounded to 10 decimal places, that's 1.5972640247.

Wait, let me verify the calculation again. Let me compute e squared more accurately. e ≈ 2.718281828459045, so e squared is 2.718281828459045 * 2.718281828459045. Let me compute that:

2.718281828459045 * 2.718281828459045. Let's do it step by step. 2.71828^2 is approximately 7.38906, but more precisely, using a calculator, e^2 is approximately 7.389056098930649772. So e² -1 is 6.389056098930649772. Divided by 4: 6.389056098930649772 /4 = 1.597264024732662443. So rounding to 10 decimal places, 1.5972640247. But let me check if the 11th decimal is 3, which is less than 5, so it stays as 1.5972640247.

Therefore, the exact answer is (e² -1)/4, and the numerical approximation is approximately 1.5972640247.
</think>

{"answer": "\\frac{e^2 - 1}{4}", "numerical_answer": "1.5972640247"}