<think>
Okay, let's tackle this integral step by step. The integral is from 0 to π/4 of [tan(x) + 2 sec²(x) + 2 tan(x) sec²(x)] divided by [tan(x) + sec²(x)] dx. Hmm, that looks a bit complicated, but maybe we can simplify the integrand first.

First, let me write down the integrand:

Numerator: tan(x) + 2 sec²(x) + 2 tan(x) sec²(x)

Denominator: tan(x) + sec²(x)

I wonder if the denominator can be simplified or if there's a substitution that would make this easier. Let's see. Let me recall that sec²(x) = 1 + tan²(x), so maybe substituting u = tan(x) could help. Let's try that.

Let u = tan(x). Then, du/dx = sec²(x), so dx = du / sec²(x). But since we have sec²(x) in the integrand, maybe this substitution will work. Let's express everything in terms of u.

First, when x = 0, u = tan(0) = 0. When x = π/4, u = 1. So the limits of integration become from 0 to 1.

Now, let's rewrite the denominator in terms of u. The denominator is tan(x) + sec²(x) = u + (1 + u²). So denominator becomes u + 1 + u² = u² + u + 1.

The numerator is tan(x) + 2 sec²(x) + 2 tan(x) sec²(x) = u + 2(1 + u²) + 2u(1 + u²). Let's expand that:

u + 2 + 2u² + 2u + 2u³. Combine like terms:

2u³ + 2u² + (u + 2u) + 2 = 2u³ + 2u² + 3u + 2.

So the integrand becomes [2u³ + 2u² + 3u + 2] / [u² + u + 1] du. But wait, we also have to account for dx. Since dx = du / sec²(x) = du / (1 + u²). Wait, hold on. Because when we do substitution u = tan(x), then du = sec²(x) dx, so dx = du / sec²(x) = du / (1 + u²). Therefore, the entire integral becomes:

∫ [ (2u³ + 2u² + 3u + 2) / (u² + u + 1) ] * [du / (1 + u²) ]

So combining the denominators, it's (2u³ + 2u² + 3u + 2) / [ (u² + u + 1)(1 + u²) ] du.

Hmm, that seems a bit messy. Maybe there's a better way to simplify the original integrand before substitution. Let me check again.

Looking back at the original integrand:

[tan(x) + 2 sec²(x) + 2 tan(x) sec²(x)] / [tan(x) + sec²(x)]

Let me factor the numerator. Let's see:

tan(x) + 2 sec²(x) + 2 tan(x) sec²(x) = tan(x)(1 + 2 sec²(x)) + 2 sec²(x)

But not sure. Alternatively, maybe factor terms with sec²(x). Let's see:

= tan(x) + 2 sec²(x) + 2 tan(x) sec²(x)

= tan(x) + 2 sec²(x) [1 + tan(x)]

Hmm, that's interesting. So the numerator can be written as tan(x) + 2 sec²(x)(1 + tan(x)). Let's see if that helps. The denominator is tan(x) + sec²(x). Let me write that as tan(x) + sec²(x) = tan(x) + 1 + tan²(x) (since sec²(x) = 1 + tan²(x)). So denominator is tan²(x) + tan(x) + 1.

So maybe if I let the denominator be expressed in terms of tan(x), and then set u = tan(x), but perhaps there's a way to split the numerator. Let's see:

Numerator: tan(x) + 2 sec²(x)(1 + tan(x)) = tan(x) + 2(1 + tan²(x))(1 + tan(x))

Let me expand that term:

2(1 + tan²(x))(1 + tan(x)) = 2(1 + tan(x) + tan²(x) + tan³(x))

So the numerator becomes:

tan(x) + 2 + 2 tan(x) + 2 tan²(x) + 2 tan³(x)

Combine like terms:

2 tan³(x) + 2 tan²(x) + (tan(x) + 2 tan(x)) + 2

= 2 tan³(x) + 2 tan²(x) + 3 tan(x) + 2

Which is the same as before. So the integrand is [2 tan³(x) + 2 tan²(x) + 3 tan(x) + 2] / [tan²(x) + tan(x) + 1]

But perhaps we can perform polynomial division here. Let's consider the numerator as a polynomial in tan(x) divided by the denominator, which is also a quadratic in tan(x). Let me set u = tan(x), so the integrand becomes [2u³ + 2u² + 3u + 2] / [u² + u + 1] du. Then, since we have to include the substitution dx = du / (1 + u²), the integral becomes:

∫ [ (2u³ + 2u² + 3u + 2) / (u² + u + 1) ] * [1 / (1 + u²) ] du

So the integrand is (2u³ + 2u² + 3u + 2) / [ (u² + u + 1)(1 + u²) ] du

Hmm, this seems complicated. Maybe we can split the fraction into partial fractions. Alternatively, perhaps perform polynomial division on the numerator and denominator.

Let me check the degrees. The numerator is degree 3, denominator is degree 4 (since (u² + u +1)(1 + u²) = u^4 + u^3 + 2u² + u +1). Wait, actually, the denominator is (u² + u +1)(u² +1) = u^4 + u^3 + u² + u^3 + u² + u + u² + u +1. Wait, no, that's not correct. Let me multiply (u² + u +1)(u² +1):

First term: u²*(u² +1) = u^4 + u²

Second term: u*(u² +1) = u^3 + u

Third term: 1*(u² +1) = u² +1

Adding all together: u^4 + u² + u^3 + u + u² +1 = u^4 + u^3 + 2u² + u +1

So denominator is u^4 + u^3 + 2u² + u +1. The numerator is 2u³ + 2u² + 3u +2. Since the denominator is of higher degree, maybe partial fractions is the way to go, but that might be tedious. Alternatively, perhaps there's a simplification I missed.

Wait, maybe before substitution, the original integrand can be simplified. Let me look again:

Original integrand: [tan(x) + 2 sec²(x) + 2 tan(x) sec²(x)] / [tan(x) + sec²(x)]

Let me factor the numerator. Let's see:

tan(x) + 2 sec²(x) + 2 tan(x) sec²(x) = tan(x)(1 + 2 sec²(x)) + 2 sec²(x)

Alternatively, group terms:

= [tan(x) + 2 tan(x) sec²(x)] + 2 sec²(x)

= tan(x)(1 + 2 sec²(x)) + 2 sec²(x)

But not sure. Alternatively, notice that the denominator is tan(x) + sec²(x). Let me write the denominator as tan(x) + 1 + tan²(x) (since sec²(x) = 1 + tan²(x)). So denominator is tan²(x) + tan(x) +1.

So denominator is a quadratic in tan(x). Let me denote u = tan(x), so denominator is u² + u +1. Then, the numerator is 2u³ + 2u² +3u +2. So perhaps perform polynomial division of numerator by denominator.

Divide 2u³ + 2u² +3u +2 by u² + u +1.

Divide 2u³ by u² to get 2u. Multiply denominator by 2u: 2u*(u² + u +1) = 2u³ + 2u² +2u. Subtract from original numerator:

(2u³ + 2u² +3u +2) - (2u³ + 2u² +2u) = (0u³ +0u² + u +2). So remainder is u +2. So the division gives 2u + (u +2)/(u² + u +1). Therefore, the integrand becomes:

[2u + (u +2)/(u² + u +1)] * [1/(1 + u²)] du

So split into two terms:

2u / (1 + u²) du + (u +2)/[(u² + u +1)(1 + u²)] du

The first integral is straightforward: 2u / (1 + u²) du. The integral of that is ln(1 + u²) + C.

The second integral is (u +2)/[(u² + u +1)(1 + u²)] du. This seems more complicated. Let's try partial fractions.

Let me denote:

(u +2)/[(u² + u +1)(u² +1)] = (Au + B)/(u² + u +1) + (Cu + D)/(u² +1)

Multiply both sides by (u² + u +1)(u² +1):

u +2 = (Au + B)(u² +1) + (Cu + D)(u² + u +1)

Expand the right-hand side:

(Au + B)(u² +1) = A u^3 + A u + B u² + B

(Cu + D)(u² + u +1) = C u^3 + C u² + C u + D u² + D u + D

Combine like terms:

= (A + C)u³ + (B + C + D)u² + (A + C + D)u + (B + D)

Set equal to left-hand side, which is u +2. Therefore, we have the equations:

For u³: A + C = 0

For u²: B + C + D = 0

For u: A + C + D = 1

For constant term: B + D = 2

Now, solve this system of equations.

From first equation: C = -A

From fourth equation: B + D = 2

From third equation: A + C + D =1. Substitute C = -A: A - A + D =1 => D =1

Then from fourth equation: B +1 =2 => B=1

From second equation: B + C + D =0. Substitute B=1, D=1, C=-A: 1 + (-A) +1 =0 => -A +2=0 => A=2

Then C = -A = -2

So the coefficients are:

A=2, B=1, C=-2, D=1

Therefore, the partial fractions decomposition is:

(2u +1)/(u² + u +1) + (-2u +1)/(u² +1)

So the second integral becomes:

∫ [ (2u +1)/(u² + u +1) + (-2u +1)/(u² +1) ] du

Let's split this into two integrals:

∫ (2u +1)/(u² + u +1) du + ∫ (-2u +1)/(u² +1) du

First integral: ∫ (2u +1)/(u² + u +1) du

Let me complete the square in the denominator: u² + u +1 = (u + 0.5)^2 + (sqrt(3)/2)^2. Alternatively, note that the derivative of the denominator is 2u +1. Wait, the numerator is 2u +1, which is exactly the derivative of the denominator. So:

Let v = u² + u +1, dv = (2u +1) du. Therefore, ∫ (2u +1)/v dv = ln|v| + C = ln(u² + u +1) + C

Second integral: ∫ (-2u +1)/(u² +1) du

Split into two terms:

-2 ∫ u/(u² +1) du + ∫ 1/(u² +1) du

First part: -2 ∫ u/(u² +1) du. Let w = u² +1, dw = 2u du, so -2)*(1/2) ∫ dw/w = -ln|w| + C = -ln(u² +1) + C

Second part: ∫1/(u² +1) du = arctan(u) + C

Putting it all together, the second integral is:

ln(u² + u +1) - ln(u² +1) + arctan(u) + C

Therefore, combining both integrals:

First integral (from the polynomial division) was 2u/(1 + u²) du = ln(1 + u²) + C

Second integral decomposed into:

ln(u² + u +1) - ln(u² +1) + arctan(u) + C

So total integral is:

ln(1 + u²) + ln(u² + u +1) - ln(u² +1) + arctan(u) + C

Simplify the logarithms:

ln(1 + u²) - ln(u² +1) cancels out, leaving ln(u² + u +1) + arctan(u) + C

Wait, that's interesting. So the entire integral simplifies to:

ln(u² + u +1) + arctan(u) + C

But u = tan(x), so substituting back:

ln(tan²x + tanx +1) + arctan(tanx) + C

But arctan(tanx) is x for x in (-π/2, π/2), which includes our interval [0, π/4]. So arctan(tanx) = x. Therefore, the antiderivative is:

ln(tan²x + tanx +1) + x + C

Now, we need to evaluate this from 0 to π/4.

Compute F(π/4) - F(0):

First, F(π/4) = ln(tan²(π/4) + tan(π/4) +1) + π/4

tan(π/4) =1, so tan²(π/4)=1. Therefore:

ln(1 +1 +1) + π/4 = ln(3) + π/4

F(0) = ln(tan²(0) + tan(0) +1) +0

tan(0)=0, so tan²(0)=0. Therefore:

ln(0 +0 +1) +0 = ln(1) +0 =0

Therefore, the definite integral is [ln(3) + π/4] -0 = ln(3) + π/4

So the exact answer is ln(3) + π/4.

Now, let's compute the numerical approximation. Let's calculate ln(3) and π/4.

ln(3) ≈ 1.0986122886681098

π ≈ 3.141592653589793, so π/4 ≈ 0.7853981634

Adding them together: 1.0986122886681098 + 0.7853981634 ≈ 1.8840104520681098

Rounded to 10 decimal places: 1.8840104521

Wait, let me check the addition:

1.0986122886681098

+0.7853981634

=1.0986122886681098 +0.7853981634

Adding:

1.0986122886681098

+0.7853981634000000

=

1.8840104520681098

Yes, so approximately 1.8840104521 when rounded to 10 decimal places.

So the exact answer is ln(3) + π/4, and the numerical approximation is approximately 1.8840104521.
</think>

{"answer": "\\ln(3) + \\frac{\\pi}{4}", "numerical_answer": 1.8840104521}