Let's compute the integral:
\[
I = \int_0^1 (x-1)^2(x+1)^2(x^2+1)^2(x^4+1)^2 \, dx
\]

Let's systematically expand and compute the integral step by step.

---

### 1. Expand \((x-1)^2(x+1)^2\)

\[
(x-1)^2(x+1)^2 = [(x-1)(x+1)]^2 = (x^2-1)^2 = x^4 - 2x^2 + 1
\]

---

### 2. Expand \((x^2+1)^2\)

\[
(x^2+1)^2 = x^4 + 2x^2 + 1
\]

---

### 3. Expand \((x^4+1)^2\)

\[
(x^4+1)^2 = x^8 + 2x^4 + 1
\]

---

### 4. Combine All Factors

Our integrand is:
\[
(x-1)^2(x+1)^2(x^2+1)^2(x^4+1)^2 = (x^4-2x^2+1)(x^4+2x^2+1)(x^8+2x^4+1)
\]

Let us first multiply the two quartic polynomials:

Let
\[
A(x) = (x^4-2x^2+1)(x^4+2x^2+1)
\]

Expand:
\[
(x^4-2x^2+1)(x^4+2x^2+1) = (x^4)(x^4+2x^2+1) - 2x^2(x^4+2x^2+1) + 1(x^4+2x^2+1)
\]

Expand each part:

- \(x^4(x^4+2x^2+1) = x^8 + 2x^6 + x^4\)
- \(-2x^2(x^4+2x^2+1) = -2x^6 - 4x^4 - 2x^2\)
- \(1(x^4+2x^2+1) = x^4 + 2x^2 + 1\)

Sum:
\[
x^8 + 2x^6 + x^4
-2x^6 -4x^4 -2x^2
+ x^4 + 2x^2 +1
\]

Combine like terms:
- \(x^8\)
- \(2x^6 - 2x^6 = 0\)
- \(x^4 - 4x^4 + x^4 = -2x^4\)
- \(-2x^2 + 2x^2 = 0\)
- \(+1\)

So,
\[
A(x) = x^8 - 2x^4 + 1
\]

So, the integrand is now:
\[
(x^8 - 2x^4 + 1)(x^8 + 2x^4 + 1)
\]

---

### 5. Multiply that by \((x^8+2x^4+1)\)

Let \(B(x) = (x^8 - 2x^4 + 1)(x^8 + 2x^4 + 1)\):

Expand:
\[
(x^8 - 2x^4 + 1)(x^8 + 2x^4 + 1)
\]
This is of the form \((a-b)(a+b) = a^2-b^2\):

Let \(a = x^8+1\), \(b=2x^4\): 
\[
(a-b)(a+b) = a^2-b^2 = (x^8+1)^2 - (2x^4)^2 = (x^8+1)^2 - 4x^8
\]
\[
= x^{16} + 2x^8 + 1 - 4x^8 = x^{16} - 2x^8 + 1
\]

Thus, the integrand is:
\[
(x^{16} - 2x^8 + 1)
\]

---

### 6. The Definite Integral

\[
I = \int_0^1 (x^{16} - 2x^8 + 1)\,dx
\]
\[
= \int_0^1 x^{16}dx - 2\int_0^1 x^8dx + \int_0^1 1dx
\]

Compute each term:

- \(\int_0^1 x^{16}dx = \left[\frac{x^{17}}{17}\right]_0^1 = \frac{1}{17}\)
- \(\int_0^1 x^{8}dx = \left[\frac{x^9}{9}\right]_0^1 = \frac{1}{9}\)
- \(\int_0^1 1dx = \left[x\right]_0^1 = 1\)

So sum:
\[
I = \frac{1}{17} - 2\left(\frac{1}{9}\right) + 1
\]
\[
= 1 + \frac{1}{17} - \frac{2}{9}
\]

Get common denominators:
LCM of 17 and 9 is 153

- \(1 = \frac{153}{153}\)
- \(\frac{1}{17} = \frac{9}{153}\)
- \(\frac{2}{9} = \frac{34}{153}\)

Sum:
\[
I = \frac{153}{153} + \frac{9}{153} - \frac{34}{153} = \frac{153+9-34}{153} = \frac{128}{153}
\]

---

### 7. Numerical Approximation

\[
\frac{128}{153} \approx 0.8366013072
\]

---

### JSON Output

```json
{"answer": "\\frac{128}{153}", "numerical_answer": "0.8366013072"}
```