# Evaluation of the definite integral $\int\limits_0^{2.0}x^{1.0-3/2}(2.0-x)^{1.0-1/2}[1-0.5x(2.0-x)]^{-1.0} dx$

First, let's simplify the expression:

$$\int\limits_0^{2.0}x^{1.0-3/2}(2.0-x)^{1.0-1/2}[1-0.5x(2.0-x)]^{-1.0} dx$$

Simplifying the exponents:
$$\int\limits_0^{2.0}x^{-1/2}(2.0-x)^{1/2}[1-0.5x(2.0-x)]^{-1.0} dx$$

## Step 1: Substitution

Let's use the substitution $x = 2u$, which gives $dx = 2du$.
When $x = 0$, $u = 0$, and when $x = 2$, $u = 1$.

Substituting:
$$\int\limits_0^{1.0}(2u)^{-1/2}(2.0-2u)^{1/2}[1-0.5(2u)(2.0-2u)]^{-1.0} \cdot 2du$$

Simplifying:
$$\int\limits_0^{1.0}2 \cdot 2^{-1/2}u^{-1/2} \cdot 2^{1/2}(1-u)^{1/2}[1-0.5 \cdot 4u(1-u)]^{-1.0}du$$
$$= 2 \cdot \int\limits_0^{1.0}u^{-1/2}(1-u)^{1/2}[1-2u(1-u)]^{-1.0}du$$

## Step 2: Recognize the beta function

The integral has the form of a beta function with an additional factor. Let's examine the term $[1-2u(1-u)]^{-1.0}$.

Note that $1-2u(1-u) = 1-2u+2u^2 = (1-u)^2 + u^2 = (1-u)^2 + u^2 = (1-u+u)^2 - 2u(1-u) = 1 - 2u(1-u)$

We can simplify: $1-2u(1-u) = (1-u)^2 + u^2$

Now our integral is:
$$2 \cdot \int\limits_0^{1.0}u^{-1/2}(1-u)^{1/2}[(1-u)^2 + u^2]^{-1.0}du$$

## Step 3: Further substitution

Let's use another substitution: $v = \frac{u}{1-u}$, which gives $u = \frac{v}{1+v}$

From this substitution:
- When $u = 0$, $v = 0$
- When $u = 1$, $v = \infty$
- $du = \frac{dv}{(1+v)^2}$

Also, $1-u = \frac{1}{1+v}$

Substituting these:
$$2 \cdot \int\limits_0^{\infty}\left(\frac{v}{1+v}\right)^{-1/2}\left(\frac{1}{1+v}\right)^{1/2}\left[\left(\frac{1}{1+v}\right)^2 + \left(\frac{v}{1+v}\right)^2\right]^{-1.0}\frac{dv}{(1+v)^2}$$

Simplifying the terms:
- $\left(\frac{v}{1+v}\right)^{-1/2} = \frac{(1+v)^{1/2}}{v^{1/2}}$
- $\left(\frac{1}{1+v}\right)^{1/2} = \frac{1}{(1+v)^{1/2}}$
- $\left[\left(\frac{1}{1+v}\right)^2 + \left(\frac{v}{1+v}\right)^2\right] = \frac{1 + v^2}{(1+v)^2}$

Plugging these in:
$$2 \cdot \int\limits_0^{\infty}\frac{(1+v)^{1/2}}{v^{1/2}} \cdot \frac{1}{(1+v)^{1/2}} \cdot \left[\frac{1 + v^2}{(1+v)^2}\right]^{-1.0}\frac{dv}{(1+v)^2}$$

Simplifying:
$$2 \cdot \int\limits_0^{\infty}\frac{1}{v^{1/2}} \cdot \frac{(1+v)^2}{(1 + v^2)} \cdot \frac{dv}{(1+v)^2}$$
$$= 2 \cdot \int\limits_0^{\infty}\frac{1}{v^{1/2}(1 + v^2)}dv$$

## Step 4: Evaluating the integral

This integral can be evaluated using standard techniques. Let $v = \tan^2(θ)$, which gives $dv = 2\tan(θ)\sec^2(θ)dθ$.

When $v = 0$, $θ = 0$, and when $v = \infty$, $θ = \pi/2$.

Also, $v^{1/2} = \tan(θ)$ and $1 + v^2 = 1 + \tan^4(θ) = \sec^4(θ)$.

Substituting:
$$2 \cdot \int\limits_0^{\pi/2}\frac{1}{\tan(θ) \cdot \sec^4(θ)} \cdot 2\tan(θ)\sec^2(θ)dθ$$
$$= 4 \cdot \int\limits_0^{\pi/2}\frac{\sec^2(θ)}{\sec^4(θ)}dθ$$
$$= 4 \cdot \int\limits_0^{\pi/2}\cos^2(θ)dθ$$

Using the half-angle formula: $\cos^2(θ) = \frac{1 + \cos(2θ)}{2}$

$$= 4 \cdot \int\limits_0^{\pi/2}\frac{1 + \cos(2θ)}{2}dθ$$
$$= 2 \cdot \int\limits_0^{\pi/2}(1 + \cos(2θ))dθ$$
$$= 2 \cdot \left[θ + \frac{\sin(2θ)}{2}\right]_0^{\pi/2}$$
$$= 2 \cdot \left[\frac{\pi}{2} + \frac{\sin(π)}{2} - 0 - \frac{\sin(0)}{2}\right]$$
$$= 2 \cdot \frac{\pi}{2} = \pi$$

Therefore, the exact value of the integral is $\pi$.

## Numerical approximation
The numerical value of $\pi$ to 10 decimal places is 3.1415926536.

{"answer": "\\pi", "numerical_answer": "3.1415926536"}