

To solve the definite integral \(\int_{0}^{2} x^{-1/2} (2-x)^{-1/2} [1-0.5x(2-x)] \, dx\), we proceed as follows:

### Step 1: Simplify the integrand and substitute variables
First, rewrite \(x(2-x)\) by completing the square:  
\(x(2-x) = 2x - x^2 = 1 - (x-1)^2\).  

This suggests the substitution \(x = 1 + \sin\theta\), where \(dx = \cos\theta \, d\theta\). The limits of integration change as follows:  
- When \(x = 0\), \(\sin\theta = -1 \implies \theta = -\pi/2\).  
- When \(x = 2\), \(\sin\theta = 1 \implies \theta = \pi/2\).  

Under this substitution:  
- \(x(2-x) = (1+\sin\theta)(1-\sin\theta) = 1 - \sin^2\theta = \cos^2\theta\),  
- \(x^{-1/2}(2-x)^{-1/2} = [x(2-x)]^{-1/2} = (\cos^2\theta)^{-1/2} = \frac{1}{\cos\theta}\) (since \(\cos\theta > 0\) for \(\theta \in (-\pi/2, \pi/2)\)),  
- The term \(1 - 0.5x(2-x) = 1 - 0.5\cos^2\theta\).  

### Step 2: Rewrite the integral in terms of \(\theta\)
Substituting these into the original integral, we get:  
\[
\int_{-\pi/2}^{\pi/2} \frac{1}{\cos\theta} \cdot \left(1 - 0.5\cos^2\theta\right) \cdot \cos\theta \, d\theta
\]  
The \(\cos\theta\) terms cancel, simplifying the integrand to \(1 - 0.5\cos^2\theta\). Thus, the integral reduces to:  
\[
\int_{-\pi/2}^{\pi/2} \left(1 - 0.5\cos^2\theta\right) d\theta
\]

### Step 3: Evaluate the simplified integral
Split the integral into two parts:  
\[
\int_{-\pi/2}^{\pi/2} 1 \, d\theta - 0.5 \int_{-\pi/2}^{\pi/2} \cos^2\theta \, d\theta
\]  

1. The first integral: \(\int_{-\pi/2}^{\pi/2} 1 \, d\theta = \left[\theta\right]_{-\pi/2}^{\pi/2} = \pi\).  

2. The second integral: Use the identity \(\cos^2\theta = \frac{1+\cos2\theta}{2}\). Then:  
\[
0.5 \int_{-\pi/2}^{\pi/2} \cos^2\theta \, d\theta = 0.5 \int_{-\pi/2}^{\pi/2} \frac{1+\cos2\theta}{2} \, d\theta = \frac{1}{4} \int_{-\pi/2}^{\pi/2} (1 + \cos2\theta) \, d\theta
\]  
The integral of \(\cos2\theta\) over \([-\pi/2, \pi/2]\) is zero (since it is an odd function over a symmetric interval). Thus:  
\[
\frac{1}{4} \int_{-\pi/2}^{\pi/2} 1 \, d\theta = \frac{1}{4} \cdot \pi = \frac{\pi}{4}
\]  

### Step 4: Combine results
The original integral equals:  
\[
\pi - \frac{\pi}{4} = \frac{3\pi}{4}
\]

### Numerical Approximation
The numerical value of \(\frac{3\pi}{4}\) is approximately \(2.3561944902\) (rounded to 10 decimal places).

{"answer": "\\frac{3\\pi}{4}", "numerical_answer": "2.3561944902"}