Let's compute the definite integral:

\[
I = \int_{0}^{1} \arctan(\sqrt{x(1-x)})\, dx
\]

### Step 1: Simplifying the Argument

Let’s denote \( y = \sqrt{x(1-x)} \). We can attempt a substitution to simplify this.

Let’s try the substitution \( x = \sin^2\theta \) where \( \theta \in [0, \frac{\pi}{2}] \):

- When \( x = 0 \), \( \theta = 0 \)
- When \( x = 1 \), \( \theta = \frac{\pi}{2} \)

Then,
\[
dx = 2\sin\theta \cos\theta\, d\theta = \sin 2\theta\, d\theta
\]
\[
x(1-x) = \sin^2\theta (1 - \sin^2\theta) = \sin^2\theta \cos^2\theta = \frac{1}{4}\sin^2 2\theta
\]
\[
\sqrt{x(1-x)} = \frac{1}{2}|\sin 2\theta| = \frac{1}{2}\sin 2\theta \ \text{on} \ [0, \pi/2]
\]

So,
\[
I = \int_{0}^{\frac{\pi}{2}} \arctan\left(\frac{1}{2}\sin 2\theta\right) \sin 2\theta\, d\theta
\]

Let’s substitute \( \phi = 2\theta \), so \( d\phi = 2d\theta \), \( \theta = 0 \implies \phi = 0 \), \( \theta = \frac{\pi}{2} \implies \phi = \pi \):

\[
I = \int_{0}^{\pi} \arctan\left(\frac{1}{2}\sin \phi\right)\frac{1}{2}\sin\phi\,d\phi
\]

Thus:
\[
I = \frac{1}{2} \int_0^\pi \arctan\left( \frac{1}{2} \sin \phi \right) \sin \phi \; d\phi
\]

---

### Step 2: Compute the Integral

Let’s let:
\[
J = \int_0^\pi \arctan\left( \frac{1}{2} \sin \phi \right) \sin \phi \; d\phi
\]

We'll compute \( J \) by parts:

Let \( u = \arctan\left(\frac{1}{2}\sin\phi\right) \), \( dv = \sin\phi\,d\phi \)

- \( du = \frac{1}{2}\cos\phi \cdot \frac{1}{1 + \left(\frac{1}{2}\sin\phi\right)^2} d\phi = \frac{\cos\phi}{2 + \sin^2\phi} d\phi \)
- \( v = -\cos\phi \)

So:
\[
J = \left[ -\arctan\left(\frac{1}{2}\sin \phi\right)\cos\phi \right]_0^\pi + \int_0^\pi \cos\phi \cdot \frac{\cos\phi}{2 + \sin^2\phi} d\phi
\]
\[
J = \left[ -\arctan\left(\frac{1}{2}\sin \phi\right)\cos\phi \right]_0^\pi + \int_0^\pi \frac{\cos^2 \phi}{2 + \sin^2\phi} d\phi
\]

At \( \phi = 0, \sin 0 = 0, \cos 0 = 1, \arctan(0) = 0 \)

At \( \phi = \pi, \sin \pi = 0, \cos \pi = -1, \arctan(0) = 0 \)

So boundary values:
\[
-0 \cdot 1 = 0 \quad \text{and} \quad - 0 \cdot (-1) = 0
\]

Boundary terms cancel.

So:
\[
J = \int_0^\pi \frac{\cos^2 \phi}{2 + \sin^2\phi} d\phi
\]

Recall \( \cos^2\phi = 1 - \sin^2\phi \):

\[
J = \int_0^\pi \frac{1 - \sin^2\phi}{2 + \sin^2\phi} d\phi = \int_0^\pi \frac{1}{2 + \sin^2\phi} d\phi - \int_0^\pi \frac{\sin^2\phi}{2 + \sin^2\phi} d\phi
\]

For the second term:
\[
\frac{\sin^2\phi}{2 + \sin^2\phi} = 1 - \frac{2}{2 + \sin^2\phi}
\]
So:
\[
\int_0^\pi \frac{\sin^2\phi}{2 + \sin^2\phi} d\phi = \int_0^\pi 1 d\phi - 2\int_0^\pi \frac{1}{2 + \sin^2\phi} d\phi = \pi - 2 \int_0^\pi \frac{1}{2 + \sin^2\phi} d\phi
\]

Therefore,
\[
J = \int_0^\pi \frac{1}{2 + \sin^2\phi} d\phi - (\pi - 2 \int_0^\pi \frac{1}{2 + \sin^2\phi} d\phi)
\]
\[
= 3\int_0^\pi \frac{1}{2 + \sin^2\phi} d\phi - \pi
\]

Recall \( I = \frac{1}{2}J \), so:
\[
I = \frac{3}{2} \int_0^\pi \frac{1}{2 + \sin^2\phi} d\phi - \frac{\pi}{2}
\]

Let’s call:
\[
A = \int_0^\pi \frac{1}{2 + \sin^2\phi} d\phi
\]
So:
\[
I = \frac{3}{2}A - \frac{\pi}{2}
\]

---

### Step 3: Evaluate \( A \)

We need to find
\[
A = \int_0^\pi \frac{1}{2 + \sin^2\phi} d\phi
\]

We can use a standard table integral:

\[
\int_0^\pi \frac{d\phi}{a + b \sin^2\phi} = \frac{\pi}{\sqrt{a(a+b)}}
\]
(for \( a > 0, a+b > 0 \))

In our case, \( a = 2, b = 1 \):

So,
\[
A = \int_0^\pi \frac{d\phi}{2 + \sin^2\phi} = \frac{\pi}{\sqrt{2 \times 3}} = \frac{\pi}{\sqrt{6}}
\]

---

Plug back into the previous result,

\[
I = \frac{3}{2} \cdot \frac{\pi}{\sqrt{6}} - \frac{\pi}{2}
\]

---

### Step 4: Simplify the Exact Answer

\[
I = \frac{3\pi}{2\sqrt{6}} - \frac{\pi}{2}
\]
Let’s factor \( \frac{\pi}{2} \):

\[
I = \frac{\pi}{2}\left( \frac{3}{\sqrt{6}} - 1 \right )
\]

\[
\frac{3}{\sqrt{6}} = \frac{3\sqrt{6}}{(\sqrt{6})^2} = \frac{3\sqrt{6}}{6} = \frac{\sqrt{6}}{2}
\]
So:
\[
I = \frac{\pi}{2}\left( \frac{\sqrt{6}}{2} - 1 \right )
\]

---

### Step 5: Calculate the Numerical Value

\[
\sqrt{6} \approx 2.449489743
\]

\[
\frac{\sqrt{6}}{2} \approx 1.224744872
\]
\[
1.224744872 - 1 = 0.224744872
\]
\[
\frac{\pi}{2} \approx 1.570796327
\]
\[
I \approx 1.570796327 \times 0.224744872 = 0.3539726535
\]

---

### Step 6: Final Answer in Requested JSON Format

```json
{"answer": "\\frac{\\pi}{2} \\left( \\frac{\\sqrt{6}}{2} - 1 \\right )", "numerical_answer": "0.3539726535"}
```