To compute the definite integral \(\int_0^{5\pi/2} \frac{dx}{2 + \cos x}\), we follow these steps:

### Step 1: Use a Substitution
We employ the standard substitution for integrals involving \(2 + \cos x\):
\[
t = \tan\left(\frac{x}{2}\right), \quad dx = \frac{2}{1 + t^2} dt, \quad \cos x = \frac{1 - t^2}{1 + t^2}.
\]
Substituting these into the integral:
\[
\int \frac{dx}{2 + \cos x} = \int \frac{\frac{2}{1 + t^2}}{2 + \frac{1 - t^2}{1 + t^2}} dt = \int \frac{2}{2(1 + t^2) + (1 - t^2)} dt = \int \frac{2}{3 + t^2} dt.
\]

### Step 2: Simplify the Integral
The integral simplifies to:
\[
\int \frac{2}{3 + t^2} dt = \frac{2}{\sqrt{3}} \arctan\left(\frac{t}{\sqrt{3}}\right) + C.
\]
Substituting back \(t = \tan\left(\frac{x}{2}\right)\):
\[
\frac{2}{\sqrt{3}} \arctan\left(\frac{\tan\left(\frac{x}{2}\right)}{\sqrt{3}}\right) + C.
\]

### Step 3: Evaluate the Definite Integral
Now, evaluate from \(0\) to \(\frac{5\pi}{2}\):
\[
\left. \frac{2}{\sqrt{3}} \arctan\left(\frac{\tan\left(\frac{x}{2}\right)}{\sqrt{3}}\right) \right|_0^{\frac{5\pi}{2}}.
\]
At \(x = 0\):
\[
\arctan\left(\frac{\tan(0)}{\sqrt{3}}\right) = \arctan(0) = 0.
\]
At \(x = \frac{5\pi}{2}\):
\[
\arctan\left(\frac{\tan\left(\frac{5\pi}{4}\right)}{\sqrt{3}}\right) = \arctan\left(\frac{1}{\sqrt{3}}\right) = \frac{\pi}{6}.
\]
However, we must account for the periodicity and behavior of \(\tan\left(\frac{x}{2}\right)\). The function \(\tan\left(\frac{x}{2}\right)\) has a period of \(2\pi\), and within the interval \([0, \frac{5\pi}{2}]\), it passes through singularities at \(x = \pi\) and \(x = 3\pi\). To handle this, we split the integral into intervals where the antiderivative is continuous:
\[
\int_0^{\frac{5\pi}{2}} \frac{dx}{2 + \cos x} = \int_0^{\pi} + \int_{\pi}^{3\pi} + \int_{3\pi}^{\frac{5\pi}{2}}.
\]
Each of these integrals evaluates to:
\[
\frac{2}{\sqrt{3}} \left[ \arctan\left(\frac{\tan\left(\frac{x}{2}\right)}{\sqrt{3}}\right) \right]_0^{\pi^-} + \frac{2}{\sqrt{3}} \left[ \arctan\left(\frac{\tan\left(\frac{x}{2}\right)}{\sqrt{3}}\right) \right]_{\pi^+}^{3\pi^-} + \frac{2}{\sqrt{3}} \left[ \arctan\left(\frac{\tan\left(\frac{x}{2}\right)}{\sqrt{3}}\right) \right]_{3\pi^+}^{\frac{5\pi}{2}}.
\]
Evaluating each:
- From \(0\) to \(\pi^-\):
  \[
  \arctan\left(\frac{\tan\left(\frac{\pi}{2}^-\right)}{\sqrt{3}}\right) = \frac{\pi}{2}, \quad \arctan(0) = 0.
  \]
- From \(\pi^+\) to \(3\pi^-\):
  \[
  \arctan\left(\frac{\tan\left(\frac{3\pi}{2}^-\right)}{\sqrt{3}}\right) = -\frac{\pi}{2}, \quad \arctan\left(\frac{\tan\left(\frac{\pi}{2}^+\right)}{\sqrt{3}}\right) = \frac{\pi}{2}.
  \]
- From \(3\pi^+\) to \(\frac{5\pi}{2}\):
  \[
  \arctan\left(\frac{\tan\left(\frac{5\pi}{4}\right)}{\sqrt{3}}\right) = \frac{\pi}{6}, \quad \arctan\left(\frac{\tan\left(\frac{3\pi}{2}^+\right)}{\sqrt{3}}\right) = -\frac{\pi}{2}.
  \]
Summing these:
\[
\frac{2}{\sqrt{3}} \left( \frac{\pi}{2} - 0 + \left(-\frac{\pi}{2} - \frac{\pi}{2}\right) + \left(\frac{\pi}{6} - \left(-\frac{\pi}{2}\right)\right) \right) = \frac{2}{\sqrt{3}} \left( \frac{\pi}{2} - \pi + \frac{2\pi}{3} \right) = \frac{2}{\sqrt{3}} \left( \frac{\pi}{6} \right) = \frac{\pi\sqrt{3}}{9}.
\]

### Step 4: Numerical Approximation
The numerical value of \(\frac{\pi\sqrt{3}}{9}\) is approximately:
\[
1.2091995761.
\]

### Final Answer
```json
{"answer": "\\frac{\\pi\\sqrt{3}}{9}", "numerical_answer": "1.2091995761"}
```