

To solve the definite integral \(\int_0^1 \left( (1 - x^{25})^{1/20} - (1 - x^{20})^{1/25} \right) \, dx\), we analyze each term separately using properties of the Beta and Gamma functions.

### Step 1: Analyze the first term \(\int_0^1 (1 - x^{25})^{1/20} \, dx\)
Let \(u = x^{25}\), so \(x = u^{1/25}\) and \(dx = \frac{1}{25} u^{-24/25} \, du\). Substituting, the integral becomes:
\[
\int_0^1 (1 - u)^{1/20} \cdot \frac{1}{25} u^{-24/25} \, du = \frac{1}{25} \int_0^1 u^{-24/25} (1 - u)^{1/20} \, du
\]
This matches the Beta function \(B(p, q) = \int_0^1 t^{p-1}(1 - t)^{q-1} \, dt\) with \(p = \frac{1}{25}\) and \(q = \frac{21}{20}\) (since \(p-1 = -\frac{24}{25}\) and \(q-1 = \frac{1}{20}\)). Using \(B(p, q) = \frac{\Gamma(p)\Gamma(q)}{\Gamma(p+q)}\), we get:
\[
\frac{1}{25} B\left( \frac{1}{25}, \frac{21}{20} \right) = \frac{1}{25} \cdot \frac{\Gamma\left( \frac{1}{25} \right) \Gamma\left( \frac{21}{20} \right)}{\Gamma\left( \frac{1}{25} + \frac{21}{20} \right)}
\]
Simplifying the argument of the denominator Gamma function:
\[
\frac{1}{25} + \frac{21}{20} = \frac{4}{100} + \frac{105}{100} = \frac{109}{100}
\]
Thus, the first integral becomes:
\[
\frac{1}{25} \cdot \frac{\Gamma\left( \frac{1}{25} \right) \Gamma\left( \frac{21}{20} \right)}{\Gamma\left( \frac{109}{100} \right)}
\]

### Step 2: Analyze the second term \(\int_0^1 (1 - x^{20})^{1/25} \, dx\)
Let \(v = x^{20}\), so \(x = v^{1/20}\) and \(dx = \frac{1}{20} v^{-19/20} \, du\). Substituting, the integral becomes:
\[
\int_0^1 (1 - v)^{1/25} \cdot \frac{1}{20} v^{-19/20} \, dv = \frac{1}{20} \int_0^1 v^{-19/20} (1 - v)^{1/25} \, dv
\]
This matches the Beta function with \(p = \frac{1}{20}\) and \(q = \frac{26}{25}\) (since \(p-1 = -\frac{19}{20}\) and \(q-1 = \frac{1}{25}\)). Using \(B(p, q) = \frac{\Gamma(p)\Gamma(q)}{\Gamma(p+q)}\), we get:
\[
\frac{1}{20} B\left( \frac{1}{20}, \frac{26}{25} \right) = \frac{1}{20} \cdot \frac{\Gamma\left( \frac{1}{20} \right) \Gamma\left( \frac{26}{25} \right)}{\Gamma\left( \frac{1}{20} + \frac{26}{25} \right)}
\]
Simplifying the argument of the denominator Gamma function:
\[
\frac{1}{20} + \frac{26}{25} = \frac{5}{100} + \frac{104}{100} = \frac{109}{100}
\]
Thus, the second integral becomes:
\[
\frac{1}{20} \cdot \frac{\Gamma\left( \frac{1}{20} \right) \Gamma\left( \frac{26}{25} \right)}{\Gamma\left( \frac{109}{100} \right)}
\]

### Step 3: Simplify using Gamma function properties
Recall \(\Gamma(z + 1) = z \Gamma(z)\). For the first term:
\[
\Gamma\left( \frac{21}{20} \right) = \Gamma\left( 1 + \frac{1}{20} \right) = \frac{1}{20} \Gamma\left( \frac{1}{20} \right)
\]
For the second term:
\[
\Gamma\left( \frac{26}{25} \right) = \Gamma\left( 1 + \frac{1}{25} \right) = \frac{1}{25} \Gamma\left( \frac{1}{25} \right)
\]
Substituting these into the integrals:
- First integral: \(\frac{1}{25} \cdot \frac{\Gamma\left( \frac{1}{25} \right) \cdot \frac{1}{20} \Gamma\left( \frac{1}{20} \right)}{\Gamma\left( \frac{109}{100} \right)} = \frac{1}{25 \cdot 20} \cdot \frac{\Gamma\left( \frac{1}{25} \right) \Gamma\left( \frac{1}{20} \right)}{\Gamma\left( \frac{109}{100} \right)}\)
- Second integral: \(\frac{1}{20} \cdot \frac{\Gamma\left( \frac{1}{20} \right) \cdot \frac{1}{25} \Gamma\left( \frac{1}{25} \right)}{\Gamma\left( \frac{109}{100} \right)} = \frac{1}{20 \cdot 25} \cdot \frac{\Gamma\left( \frac{1}{20} \right) \Gamma\left( \frac{1}{25} \right)}{\Gamma\left( \frac{109}{100} \right)}\)

### Step 4: Compute the difference
The two integrals are identical, so their difference is:
\[
\int_0^1 \left( (1 - x^{25})^{1/20} - (1 - x^{20})^{1/25} \right) \, dx = 0
\]

### Numerical Approximation
The exact value is \(0\), so the numerical approximation is \(0.0000000000\).

{"answer": "0", "numerical_answer": "0.0000000000"}