Let's break down the integral step by step.

Given:
\[
I = \int_{0}^{2} x^{-1/2}\,(2-x)^{-1/2}\,(1+0.5x)^{-2}\,T_2\left(\sqrt{1+0.5x}\right)\, dx
\]
where \( T_2(x) \) is the 2nd-degree Chebyshev polynomial,
\[
T_2(x) = 2x^2 - 1
\]
So,
\[
T_2(\sqrt{1+0.5x}) = 2(1+0.5x) - 1 = 2 + x - 1 = 1 + x
\]

Now substitute into the original integral:
\[
I = \int_{0}^{2} \frac{x^{-1/2}(2-x)^{-1/2}(1+x)}{(1+0.5x)^2} dx
\]

Let’s try the substitution \( x = 2\sin^2\theta \), with \( \theta \in [0, \frac{\pi}{2}] \):
- \( x = 2 \sin^2\theta \implies dx = 4\sin\theta\cos\theta\, d\theta = 2\sin 2\theta\, d\theta \)
- \( x^{-1/2} = (2 \sin^2\theta)^{-1/2} = \frac{1}{\sqrt{2}\,\sin\theta} \)
- \( 2-x = 2 (1-\sin^2\theta) = 2\cos^2\theta \implies (2-x)^{-1/2} = \frac{1}{\sqrt{2}\,\cos\theta} \)
- \( 1+0.5x = 1+0.5\cdot2\sin^2\theta = 1 + \sin^2\theta \)
- \( 1+x = 1 + 2\sin^2\theta \)

Plug in:
\[
I = \int_{\theta=0}^{\pi/2}
    \frac{1}{\sqrt{2}\sin\theta} \cdot \frac{1}{\sqrt{2}\cos\theta}
    \cdot \frac{1 + 2\sin^2\theta}{(1+\sin^2\theta)^2}
    \cdot 2\sin2\theta\, d\theta
\]

Simplifying step by step:
- \( \frac{1}{\sqrt{2}\sin\theta} \cdot \frac{1}{\sqrt{2}\cos\theta} = \frac{1}{2\sin\theta\cos\theta} \)
- \( 2\sin2\theta = 4\sin\theta\cos\theta \)

So,

\[
I = \int_{0}^{\pi/2}
    \frac{1 + 2\sin^2\theta}{(1+\sin^2\theta)^2}
    \cdot \frac{4\sin\theta\cos\theta}{2\sin\theta\cos\theta}\, d\theta
  = \int_{0}^{\pi/2} \frac{1 + 2\sin^2\theta}{(1+\sin^2\theta)^2} \cdot 2\, d\theta
\]

\[
I = 2 \int_{0}^{\pi/2} \frac{1 + 2\sin^2\theta}{(1+\sin^2\theta)^2} d\theta
\]

Now, expand the numerator:

\[
1 + 2\sin^2\theta = \big[1+\sin^2\theta\big] + \sin^2\theta
\implies
I = 2\int_{0}^{\pi/2} \frac{1+\sin^2\theta}{(1+\sin^2\theta)^2}\,d\theta
+ 2\int_{0}^{\pi/2} \frac{\sin^2\theta}{(1+\sin^2\theta)^2}\, d\theta
\]

But \( \frac{1+\sin^2\theta}{(1+\sin^2\theta)^2} = \frac{1}{1+\sin^2\theta} \).

So,

\[
I = 2\int_{0}^{\pi/2} \frac{1}{1+\sin^2\theta}\, d\theta
+ 2\int_{0}^{\pi/2} \frac{\sin^2\theta}{(1+\sin^2\theta)^2}\, d\theta
\]

Let’s call the first integral \( A \) and the second \( B \):

\[
A = \int_{0}^{\pi/2} \frac{1}{1+\sin^2\theta} d\theta
\]
\[
B = \int_{0}^{\pi/2} \frac{\sin^2\theta}{(1+\sin^2\theta)^2} d\theta
\]

But look:
\[
B = \int_{0}^{\pi/2} \frac{\sin^2\theta}{(1+\sin^2\theta)^2} d\theta
= \int_{0}^{\pi/2} \left[ \frac{1}{1+\sin^2\theta} - \frac{1}{(1+\sin^2\theta)^2} \right] d\theta
\]

So:
\[
I = 2A + 2B = 2A + 2\left(A - \int_{0}^{\pi/2} \frac{1}{(1+\sin^2\theta)^2} d\theta\right)
= 4A - 2C
\]
where
\[
C = \int_{0}^{\pi/2} \frac{1}{(1+\sin^2\theta)^2} d\theta
\]

So,
\[
I = 4A - 2C
\]

Let’s find \( A \) and \( C \).

---

### Step 1: Compute \( A = \int_{0}^{\pi/2} \frac{d\theta}{1+\sin^2\theta} \)

From standard integrals (see Gradshteyn & Ryzhik 3.621.2), for \( a > 0 \):
\[
\int_{0}^{\pi/2} \frac{d\theta}{a^2+\sin^2\theta} = \frac{\pi}{2 a\sqrt{a^2-1}}
\]
But in our case \( a^2 = 1 \), so that formula doesn't work, but there is a special evaluation:

Alternatively, let's calculate \( A \).

Let’s try substituting \( \sin^2\theta = y \implies \theta \in [0, \pi/2], y \in [0, 1] \):
- When \( \theta = 0, y = 0 \)
- When \( \theta = \pi/2, y = 1 \)
- \( d\theta = \frac{dy}{2\sin\theta\cos\theta} = \frac{dy}{\sin2\theta} \)

But that's clumsy.

Alternatively, let's recall that

\[
A = \int_{0}^{\pi/2} \frac{d\theta}{1+\sin^2\theta}
\]
This is evaluated as:

By substitution \( \sin\theta = t \), \( \theta = \arcsin t \), \( d\theta = \frac{dt}{\sqrt{1 - t^2}} \):

\[
A = \int_{t=0}^{t=1} \frac{1}{1 + t^2} \cdot \frac{dt}{\sqrt{1-t^2}}
\]

However, this is a standard integral and it is known:
\[
\int_{0}^{\pi/2} \frac{d\theta}{1 + k^2 \sin^2\theta} = \frac{\pi}{2\sqrt{1 + k^2}},\quad k > -1
\]
Set \( k = 1 \):
\[
A = \frac{\pi}{2\sqrt{2}}
\]

---

### Step 2: Compute \( C = \int_{0}^{\pi/2} \frac{d\theta}{(1+\sin^2\theta)^2} \)

Similarly, the standard result (Gradshteyn & Ryzhik 3.621.3) gives:

\[
\int_{0}^{\pi/2} \frac{d\theta}{(1+k^2 \sin^2\theta)^2}
= \frac{\pi(2 + k^2)}{4(1+k^2)^{3/2}}
\]
For \( k = 1 \):
\[
C = \frac{\pi (2+1)}{4 (1+1)^{3/2}}
= \frac{3\pi}{4 \cdot (2)^{3/2}} = \frac{3\pi}{4 \cdot 2\sqrt{2}} = \frac{3\pi}{8\sqrt{2}}
\]

---

### Step 3: Substitute back into the formula for \( I \):

\[
I = 4A - 2C = 4 \cdot \frac{\pi}{2\sqrt{2}} - 2 \cdot \frac{3\pi}{8\sqrt{2}}
= \frac{2\pi}{\sqrt{2}} - \frac{3\pi}{4\sqrt{2}}
\]
\[
= \frac{2\pi}{\sqrt{2}} - \frac{3\pi}{4\sqrt{2}}
= \frac{8\pi - 3\pi}{4\sqrt{2}}
= \frac{5\pi}{4\sqrt{2}}
\]

---

### Step 4: Numerical approximation

\[
\frac{5\pi}{4\sqrt{2}} \approx \frac{5 \times 3.1415926536}{4 \times 1.4142135624} \approx \frac{15.7079632678}{5.6568542496} \approx 2.7780109780
\]

---

### Final Answer

```json
{"answer": "\\frac{5\\pi}{4\\sqrt{2}}", "numerical_answer": "2.7780109780"}
```