Let's solve the integral:
\[
I = \int_0^2 x \arcsin\left(0.5 \sqrt{x(2-x)}\right) dx
\]

### Step 1: Substitution

Let’s try substituting \(x = 1 - \cos\theta\).

When \(x = 0\), \(\cos\theta = 1 \implies \theta = 0\).

When \(x = 2\), \(\cos\theta = -1 \implies \theta = \pi\).

Calculate \(x(2-x)\):
\[
x(2-x) = (1-\cos\theta)(2-(1-\cos\theta)) = (1-\cos\theta)(1+\cos\theta) = 1 - \cos^2\theta = \sin^2\theta
\]
So,
\[
0.5\sqrt{x(2-x)} = 0.5 \sin\theta
\]

The argument of \(\arcsin()\) becomes \(0.5\sin\theta\), and
\[
dx = \sin\theta d\theta
\]

Also,
\[
x = 1 - \cos\theta
\]

Substituting everything:
\[
I = \int_{0}^{\pi} (1-\cos\theta)\cdot \arcsin\left(0.5\sin\theta\right) \cdot \sin\theta d\theta
\]

Expanding:
\[
I = \int_{0}^{\pi} \arcsin(0.5\sin\theta)(\sin\theta - \sin\theta \cos\theta)d\theta
\]

Break into two integrals:
\[
I = I_1 - I_2
\]
where
\[
I_1 = \int_{0}^{\pi} \arcsin(0.5\sin\theta)\sin\theta\, d\theta
\]
\[
I_2 = \int_{0}^{\pi} \arcsin(0.5\sin\theta)\sin\theta\cos\theta\, d\theta
\]

---

### Step 2: Evaluate the First Integral \(I_1\)

Let’s use substitution \(u = \arcsin(0.5\sin\theta)\).

Let’s instead try to evaluate the integral via another substitution.

Alternatively, let’s keep the calculations as is and try to evaluate the sum (since this is a well-behaved function over [0, π]) and maybe recognize a pattern or use further substitutions.

Alternatively, swap back to \(x\) and attempt integration by parts:

Let’s set:
\[
u = \arcsin\left(0.5\sqrt{x(2-x)}\right), \quad dv = x dx
\]
But differentiating \(u\) seems messy. Let's attempt a different substitution.

Alternatively, let's try to compute the integral numerically and compare.

#### Let’s do a trigonometric substitution in the original variable.

Let \(x = 1 - \cos\theta\), as before.
\[
I = \int_{0}^{\pi} \arcsin(0.5\sin\theta)(\sin\theta - \sin\theta\cos\theta)d\theta
\]

Let’s note:

- \(\sin\theta - \sin\theta\cos\theta = \sin\theta(1 - \cos\theta)\)
- \(1-\cos\theta = x\), so it matches \(x\) in the original.

But further, consider the symmetry of the functions.

Let’s attempt change of variable within the θ integral, perhaps with θ → π−θ. Compute \(I_1\) and \(I_2\) separately.

#### Compute \(I_1\)

Let’s change variable θ → π−θ:
- \(\sin(π−θ) = \sin\theta\)
- \(\arcsin(0.5\sin(π−θ)) = \arcsin(0.5\sin\theta)\)

So the integrand is symmetric about π/2; integrating over [0,π] is twice integrating over [0,π/2].

So:
\[
I_1 = 2\int_0^{\pi/2} \arcsin(0.5\sin\theta)\sin\theta d\theta
\]

Similarly, for \(I_2\), observe that:
\[
\sin\theta\cos\theta = \frac{1}{2}\sin 2\theta
\]
So,
\[
I_2 = \int_0^{\pi} \arcsin(0.5\sin\theta)\cdot\frac{1}{2}\sin 2\theta\, d\theta
\]

But \(\sin 2\theta\) is antisymmetric about π/2, but \(\arcsin(0.5\sin\theta)\) is symmetric, so the product is antisymmetric: integrating over [0,π] yields zero.

But let's check:
Let’s denote \(f(\theta) = \arcsin(0.5\sin\theta)\).

Let’s calculate \(I_2\):
\[
I_2 = \int_{0}^{\pi} f(\theta) \cdot \frac{1}{2} \sin 2\theta d\theta
\]

Under θ → π−θ:
- \(\sin 2(\pi-\theta) = -\sin 2\theta\)
- \(f(\pi-\theta) = f(\theta)\)

Thus, \(f(\theta)\sin 2\theta\) is antisymmetric over [0, π], so its integral is 0.

Therefore,
\[
I = I_1
\]

So,
\[
I = \int_0^{\pi} \arcsin(0.5\sin\theta)\sin\theta d\theta
\]

---

### Step 3: Back-Substitution

Now, let’s try to express \(I\) in the original variable.

Alternate idea: Let's use substitution \(x = \sin\phi\), \(x \in [0,1]\) (but our upper bound is 2), so perhaps not expedient.

Let’s attempt direct integration by parts in θ variable.

Set:
- Let \(u = \arcsin(0.5\sin\theta)\),
- \(dv = \sin\theta d\theta\),
then \(v = -\cos\theta\).

So:
\[
I = uv\Big|_0^{\pi} - \int_0^{\pi} v du = \left[-\arcsin(0.5\sin\theta)\cos\theta \right]_{0}^{\pi} + \int_0^{\pi} \cos\theta \cdot \frac{d}{d\theta}\arcsin(0.5\sin\theta) d\theta
\]

Check the boundary terms:

At θ = 0:
- \(\sin 0 = 0\), so \(\arcsin(0) = 0\), \(\cos 0 = 1\), so term is 0.

At θ = π:
- \(\sinπ=0\), so \(\arcsin(0)=0\), \(\cos π = -1\), so term is also 0.

Thus, the boundary terms are zero.

Thus,
\[
I = \int_0^{\pi} \cos\theta \frac{d}{d\theta} \arcsin[0.5\sin\theta] d\theta
\]
Compute the derivative:

Let \(f(\theta) = 0.5\sin\theta\),
\[
\frac{d}{d\theta} \arcsin(f(\theta)) = \frac{f'(\theta)}{ \sqrt{1 - [f(\theta)]^2 } }
\]
\[
f(\theta) = 0.5\sin\theta,\qquad f'(\theta) = 0.5\cos\theta
\]
\[
1 - [0.5\sin\theta]^2 = 1 - 0.25\sin^2\theta
\]

So,
\[
I = \int_0^{\pi} \cos\theta \cdot \frac{0.5\cos\theta}{\sqrt{1 - 0.25\sin^2\theta}} d\theta = 0.5\int_0^{\pi} \cos^2\theta \cdot \frac{d\theta}{\sqrt{1-0.25\sin^2\theta}}
\]

Let’s write \(\cos^2\theta = \frac{1 + \cos 2\theta}{2}\):

\[
I = 0.5 \int_0^{\pi} \frac{1 + \cos 2\theta}{2} \cdot \frac{d\theta}{\sqrt{1-0.25\sin^2\theta}}
= \frac{1}{4} \int_0^{\pi} \frac{d\theta}{\sqrt{1-0.25\sin^2\theta}}
+ \frac{1}{4} \int_0^{\pi} \frac{\cos 2\theta d\theta}{\sqrt{1-0.25\sin^2\theta}}
\]

Both are classic elliptic integrals.

Set \(k^2 = 0.25 \implies k = \frac{1}{2}\).

Recall that the complete elliptic integrals are
\[
K(k) = \int_0^{\pi/2} \frac{d\theta}{\sqrt{1 - k^2 \sin^2\theta}}
\]
\[
E(k) = \int_0^{\pi/2} \sqrt{1 - k^2 \sin^2\theta} d\theta
\]

But our integrals go from \(0\) to \(\pi\). So,

\[
\int_0^{\pi} \frac{d\theta}{\sqrt{1 - k^2 \sin^2\theta}} = 2K(k)
\]

For the other term:
\[
\int_0^{\pi} \frac{\cos 2\theta d\theta}{\sqrt{1 - k^2\sin^2\theta}}
\]

Recall that
\[
\int_0^{\pi} \frac{\cos n\theta\,d\theta}{\sqrt{1 - k^2\sin^2\theta}}
= 
\frac{2\pi}{P(k)} \cos\left(\frac{n\pi}{2}\right)
\]
But more generally, let's recall
\[
\int_0^{\pi} \frac{\cos 2\theta d\theta}{\sqrt{1 - k^2\sin^2\theta}}
= 2\int_0^{\pi/2} \frac{\cos 2\theta d\theta}{\sqrt{1 - k^2\sin^2\theta}}
\]

And in Abramowitz & Stegun (17.4.17): 
\[
\int_0^{\pi/2} \frac{\cos 2\theta d\theta}{\sqrt{1 - k^2\sin^2\theta}}
= \frac{E(k) - (1 - k^2)K(k)}{k^2}
\]

So doubling, we get:
\[
\int_0^{\pi} \frac{\cos 2\theta d\theta}{\sqrt{1 - k^2\sin^2\theta}}
= \frac{2}{k^2}[E(k) - (1 - k^2)K(k)]
\]

With \(k = 1/2\), \(k^2 = 1/4\):

\[
\int_0^{\pi} \frac{\cos 2\theta d\theta}{\sqrt{1 - 0.25\sin^2\theta}}
= 8 [E(1/2) - (1 - 1/4)K(1/2)] = 8[E(1/2) - (3/4)K(1/2)]
\]

Bring it all together:

\[
I = \frac{1}{4} \left[ 2K\left( \frac{1}{2} \right) + 8(E(1/2) - (3/4)K(1/2)) \right]
\]
\[
= \frac{1}{2} K\left( \frac{1}{2} \right) + 2\left( E\left( \frac{1}{2} \right) - \frac{3}{4} K\left( \frac{1}{2} \right) \right)
\]
\[
= 2 E\left( \frac{1}{2} \right) + \frac{1}{2} K\left( \frac{1}{2} \right) - \frac{3}{2} K\left( \frac{1}{2} \right)
\]
\[
= 2 E\left( \frac{1}{2} \right) - K\left( \frac{1}{2} \right)
\]

Therefore, the exact answer is:
\[
I = 2 E\left( \frac{1}{2} \right) - K\left( \frac{1}{2} \right)
\]

---

### Step 4: Numerical Evaluation

Using standard values:
- \(K(1/2) \approx 1.6857503548\)
- \(E(1/2) \approx 1.4674622093\)

So,
\[
I \approx 2 \times 1.4674622093 - 1.6857503548 = 2.9349244186 - 1.6857503548 = 1.2491740638
\]

---

### Step 5: Final Answer in JSON

```json
{"answer": "2 E\\left(\\frac{1}{2}\\right) - K\\left(\\frac{1}{2}\\right)", "numerical_answer": "1.2491740638"}
```