Let's solve the definite integral
\[
I = \int_0^2 x H_3\left(\sqrt{x(2-x)}\right) dx,
\]
where \( H_3(y) \) is the third Hermite polynomial. Recall:
\[
H_3(y) = 8y^3 - 12y.
\]

**Step 1: Substitution**

Let \( y = \sqrt{x(2-x)} \Rightarrow y^2 = x(2-x) \Rightarrow x^2 - 2x + y^2 = 0 \).

Solve for \( x \):
\[
x^2 - 2x + y^2 = 0 \implies x = 1 \pm \sqrt{1-y^2}.
\]
Since as \( x \) goes from 0 to 2, \( y \) goes from 0 to \(\sqrt{2}\), but let's check endpoints:

- At \( x = 0 \): \( y = 0 \).
- At \( x = 2 \): \( y = 0 \).
- Maximum at \( x = 1 \): \( y = \sqrt{1(2-1)} = 1 \).

So the substitution covers \( y \in [0, 1] \) as \( x \in [0, 2] \).

Let's solve for \( x \) in this range:
\[
x = 1 - \sqrt{1-y^2},\ 1+\sqrt{1-y^2}.
\]
At \( x = 0 \): \( y = 0 \to x = 1-1 = 0 \); at \( x = 1 \): \( y = 1 \to x = 1 \pm 0 = 1 \); at \( x = 2 \): \( y = 0 \to x = 1+1 = 2 \).

So, as \( x \) goes from 0 to 1, \( y \) goes from 0 to 1 (with smaller root), as \( x \) goes from 1 to 2, \( y \) goes from 1 to 0 (with larger root).

Alternatively, parameterize:
Let \( x = 1 + \cos\theta \), \( 0 \leq \theta \leq \pi \).

Then,
\[
x(2-x) = (1 + \cos\theta)(2 - (1+\cos\theta)) = (1 + \cos\theta)(1 - \cos\theta) = 1 - \cos^2\theta = \sin^2\theta.
\]
So, \( y = |\sin\theta| \). Over \( \theta \in [0,\pi] \), \( y = \sin\theta \in [0,1] \).

When \( \theta = 0 \): \( x = 2, y = 0 \), \(\theta = \pi/2\): \( x = 1, y = 1 \), \(\theta = \pi\): \( x = 0, y = 0 \).

So \( x \) decreases from 2 to 0 as \(\theta\) goes from 0 to \(\pi\).

The Jacobian:
\[
dx = -\sin\theta d\theta
\]
But as \(\theta\) increases from 0 to \(\pi\), \( dx \) is negative, flipping the order. So integrate from \(\theta = \pi\) to \(\theta = 0\), or flip the sign.

So,
\[
I = \int_{\theta = \pi}^0 x H_3(y) dx = -\int_{0}^{\pi} x H_3(y) dx
\]
But let's set positive direction: \( x(\theta) = 1+\cos\theta \), \( y(\theta) = \sin\theta \), \( dx = -\sin\theta d\theta \).

Then,
\[
I = \int_{x=0}^{x=2} x H_3(\sqrt{x(2-x)}) dx = \int_{\theta=\pi}^{\theta=0} x(\theta) H_3(y(\theta)) dx
\]

But with \( dx = -\sin\theta\, d\theta \), we can write

\[
I = \int_{\theta=0}^{\theta=\pi} x(\theta) H_3(y(\theta)) \sin\theta\, d\theta
\]

Compute:
- \( x = 1+\cos\theta \)
- \( y = \sin\theta \)
- \( H_3(y) = 8\sin^3\theta - 12\sin\theta \)

So:

\[
I = \int_0^{\pi} (1+\cos\theta)\left[8\sin^3\theta - 12\sin\theta\right] \sin\theta d\theta
\]
\[
= \int_0^{\pi} (1+\cos\theta)[8\sin^4\theta - 12\sin^2\theta ] d\theta
\]
\[
= 8\int_0^{\pi} (1+\cos\theta)\sin^4\theta d\theta - 12\int_0^{\pi} (1+\cos\theta)\sin^2\theta d\theta
\]
Let us compute each term separately.

---

**Step 2: Compute Each Integral**

Let \( A = \int_0^\pi (1+\cos\theta)\sin^4\theta d\theta \)
Let \( B = \int_0^\pi (1+\cos\theta)\sin^2\theta d\theta \)

So,
\[
I = 8A - 12B,
\]
Let's evaluate \( A \):

**Compute \( A \):**

\[
A = \int_0^{\pi} \sin^4\theta d\theta + \int_0^{\pi} \cos\theta \sin^4\theta d\theta = A_1 + A_2
\]

Recall:

\[
\sin^4\theta = \frac{3}{8} - \frac{1}{2} \cos 2\theta + \frac{1}{8}\cos 4\theta
\]
So,

\[
A_1 = \int_0^{\pi} \sin^4\theta d\theta = \frac{3}{8} \pi - \frac{1}{2} \int_0^{\pi} \cos 2\theta d\theta + \frac{1}{8} \int_0^{\pi} \cos 4\theta d\theta
\]

- \(\int_0^{\pi} \cos 2\theta d\theta = [\frac{1}{2} \sin 2\theta]_0^{\pi} = 0\)
- \(\int_0^{\pi} \cos 4\theta d\theta = [\frac{1}{4} \sin 4\theta]_0^{\pi} = 0\)

So,

\[
A_1 = \frac{3}{8} \pi
\]

Now \( A_2 = \int_0^{\pi} \cos\theta \sin^4\theta d\theta \).

Let’s compute \( \int_0^{\pi} \cos\theta \sin^4\theta d\theta \):

Let’s use substitution \( u = \sin\theta \implies du = \cos\theta d\theta \).
When \(\theta = 0, u=0\), \(\theta = \pi, u=0\).

So,

\[
A_2 = \int_{\theta=0}^{\pi} \sin^4\theta \cos\theta d\theta = \int_{u=0}^{0} u^4 du = 0
\]
But let's check this, as the upper and lower limits are both 0, but the path from \(\theta=0\) to \(\theta=\pi\) goes through \(u=1\) at \(\theta = \pi/2\). So the integral should be zero because the path returns to 0, i.e., the area under the curve cancels itself.

But let's double-check by integrating by parts or with the substitution.

But actually, let's recall that

\[
\int_0^\pi \cos\theta \sin^n\theta d\theta = 0,\ \text{for even } n
\]
But let's formally check by integrating \( \sin^4\theta \cos\theta d\theta \).

Let’s compute:

Let’s do substitution \( u = \sin\theta \implies du = \cos\theta d\theta \), \( u=0 \) at \( \theta = 0 \), \( u=0 \) at \( \theta = \pi \).

\[
A_2 = \int_0^{\pi} \sin^4\theta \cos\theta d\theta = \int_{u=0}^{u=0} u^4 du = 0
\]

So, \( A_2 = 0 \).

Hence,

\[
A = \frac{3}{8}\pi
\]

---

Now compute \( B \):

\[
B = \int_0^\pi (1+\cos\theta)\sin^2\theta d\theta = \int_0^\pi \sin^2\theta d\theta + \int_0^\pi \cos\theta \sin^2\theta d\theta = B_1 + B_2
\]

First,

\[
\sin^2\theta = \frac{1 - \cos 2\theta}{2}
\]
So,

\[
B_1 = \int_0^\pi \frac{1}{2} d\theta - \int_0^\pi \frac{1}{2} \cos 2\theta d\theta
= \frac{\pi}{2} - \frac{1}{2} \int_0^\pi \cos 2\theta d\theta
\]

We have already calculated: \(\int_0^\pi \cos 2\theta d\theta = 0\), so

\[
B_1 = \frac{\pi}{2}
\]

Now,

\[
B_2 = \int_0^\pi \cos\theta \sin^2\theta d\theta
\]
Let’s use:
Substitute \( u = \sin\theta \implies du = \cos\theta d\theta \), \( u=0 \) at \( \theta = 0 \), \( u=0 \) at \( \theta = \pi \),

So,
\[
B_2 = \int_{u=0}^{u=0} u^2 du = 0
\]

So,
\[
B = \frac{\pi}{2}
\]

---

So the integral

\[
I = 8A - 12B = 8 \cdot \frac{3}{8}\pi - 12 \cdot \frac{\pi}{2} = 3\pi - 6\pi = -3\pi
\]

---

**Step 3: Numerical Approximation**

\[
I = -3\pi \approx -3 \times 3.1415926536 = -9.4247779608
\]

---

**Final Answer (in JSON format):**

```json
{"answer": "-3\\pi", "numerical_answer": "-9.4247779608"}
```