

To calculate the definite integral \(\int_0^\infty \frac{1}{e^x + 1} \, dx\), we proceed as follows:

### Step 1: Substitution
Let \( t = e^x \). Then \( dt = e^x \, dx \), so \( dx = \frac{dt}{t} \). When \( x = 0 \), \( t = 1 \), and as \( x \to \infty \), \( t \to \infty \). The integral transforms to:
\[
\int_1^\infty \frac{1}{t + 1} \cdot \frac{dt}{t} = \int_1^\infty \frac{1}{t(t + 1)} \, dt
\]

### Step 2: Partial Fraction Decomposition
Decompose \(\frac{1}{t(t + 1)}\) into partial fractions:
\[
\frac{1}{t(t + 1)} = \frac{1}{t} - \frac{1}{t + 1}
\]

### Step 3: Integrate Term by Term
Integrate the decomposed expression:
\[
\int_1^\infty \left( \frac{1}{t} - \frac{1}{t + 1} \right) dt = \left[ \ln|t| - \ln|t + 1| \right]_1^\infty
\]

### Step 4: Evaluate the Limits
As \( t \to \infty \), \( \ln(t) - \ln(t + 1) = \ln\left( \frac{t}{t + 1} \right) \to \ln(1) = 0 \). At \( t = 1 \):
\[
\ln(1) - \ln(2) = 0 - \ln(2) = -\ln(2)
\]

Thus, the integral evaluates to:
\[
0 - (-\ln(2)) = \ln(2)
\]

### Numerical Approximation
The natural logarithm of 2 is approximately \( 0.69314718056 \). Rounded to 10 decimal places, this is \( 0.6931471806 \).

{"answer": "\(\ln 2\)", "numerical_answer": "0.6931471806"}