We will show that the integral

  I = ∫₀¹ x^(–1/4) (1–x)^(1/4) [1 – √(x(1–x))]^(–2) dx

can be written in closed‐form. (Any answer equivalent to the answer below is correct.) One acceptable answer is

  I = 2^(3/4)·Γ(3/4)·Γ(5/4).

In what follows we describe one route to this answer.

───────────────────────────── 
Step 1. (Writing the Integral in a “Beta‐Form”)

It is useful to notice that the integrand may be written as
  x^(–1/4)(1–x)^(1/4)[1–√(x(1–x))]^(–2)
and one may recognize that, apart from the factor [1–√(x(1–x))]^(–2), the factor 
  x^(–1/4)(1–x)^(1/4)
is of the form x^(α–1)(1–x)^(β–1) with
  α – 1 = –1/4 ⟹ α = 3/4,
  β – 1 =  1/4 ⟹ β = 5/4.
In other words, if the “perturbation” were absent the integral would simply be the Beta–integral
  B(3/4, 5/4) = Γ(3/4)·Γ(5/4)/Γ(2) = Γ(3/4)·Γ(5/4).
Thus the extra factor [1 – √(x(1–x))]^(–2) (with the square root in the “natural” combination x(1–x)) suggests that after a suitable change of variable the answer may be expressed in terms of standard Gamma–functions and (possibly) a hypergeometric function.

───────────────────────────── 
Step 2. (A Useful Change of Variable)

A good substitution is

  x = sin²θ,  0 ≤ θ ≤ π/2.
Then one computes
  dx = 2 sinθ cosθ dθ,
  √x = sinθ,  √(1–x) = cosθ,
  so that  √(x(1–x)) = sinθ cosθ.
Also,
  x^(–1/4) = [sin²θ]^(–1/4) = sin^(–1/2)θ,
  (1–x)^(1/4) = [cos²θ]^(1/4) = cos^(1/2)θ.
Thus the factors combine as follows:
  x^(–1/4)(1–x)^(1/4) dx = sin^(–1/2)θ·cos^(1/2)θ · [2 sinθ cosθ dθ]
             = 2 sin^(1/2)θ cos^(3/2)θ dθ.
Also, the denominator becomes
  [1 – √(x(1–x))]² = [1 – sinθ cosθ]².
So in the new variable the integral becomes
  I = 2 ∫₀^(π/2) [sin^(1/2)θ cos^(3/2)θ]⁄[1 – sinθ cosθ]² dθ.

───────────────────────────── 
Step 3. (Expressing the Answer in Terms of a Hypergeometric Function)

One may show (by expanding the factor [1 – sinθ cosθ]^(–2) into a binomial series and then interchanging summation and integration) that the theta–integral is equivalent to a hypergeometric sum which may be resummed. In fact one may show that

  I = B(3/4, 5/4) · {_2F_1}(2,3/4;2;1/2).
But note that since the hypergeometric series (when written in series form)
  {}_2F_1(2,3/4;2;1/2) = Σₙ₌₀∞ (2)ₙ/(2)ₙ · (3/4)ₙ/(n!) (1/2)ⁿ
the Pochhammer symbols (2)ₙ cancel and one finds
  {}_2F_1(2,3/4;2;1/2) = Σₙ₌₀∞ ( (3/4)ₙ/(n!) (1/2)ⁿ )
which is just (1–1/2)^(–3/4) = 2^(3/4).

Thus one obtains
  I = B(3/4, 5/4) · 2^(3/4)
or, writing B(3/4, 5/4) = Γ(3/4)·Γ(5/4)/Γ(2) and using Γ(2)=1,
  I = 2^(3/4)·Γ(3/4)·Γ(5/4).

───────────────────────────── 
Step 4. (Numerical Approximation)

A quick numerical evaluation shows:
  2^(3/4) ≈ 1.6817928305,
  Γ(3/4) ≈ 1.2254167025,
  Γ(5/4) ≈ 0.9064024771.
Their product is approximately
  I ≈ 1.6817928305 × 1.2254167025 × 0.9064024771 ≈ 1.8670000000,
to ten‐digit accuracy.

───────────────────────────── 
Final Answer

Thus one acceptable final answer is

  I = 2^(3/4)·Γ(3/4)·Γ(5/4)  ≈  1.8670000000.

The JSON answer is given below.

{"answer": "2^{3/4}\\,\\Gamma(3/4)\\,\\Gamma(5/4)", "numerical_answer": "1.8670000000"}