We will show that the answer can be written in closed‐form. (Any answer equivalent to the answer below is correct.) In what follows a change of variable transforms the original integral

  I = ∫₀¹ x⋅ln(√(x(1–x)) + √(1+x(1–x))) dx

into an integral that may be evaluated in closed‐form in terms of logarithms and dilogarithms.

Step 1. Begin by writing the integral in “symmetric form”. The substitution

  x = u + ½       (so that u = x – ½)
  dx = du

transforms the integration limits: when x = 0, u = –½; when x = 1, u = +½. Also note that
  x(1–x) = (u+½)(½–u) = ¼ – u².
Thus the integrand becomes
  x ln(√(x(1–x)) + √(1+x(1–x)))
   = (u+½) ln ( √(¼–u²) + √(1+¼–u²) )
   = (u+½) ln ( √(¼–u²) + √(5/4–u²) ).

So
  I = ∫₋¹⁄₂^(+1⁄2) (u+½) ln ( √(¼–u²) + √(5/4–u²) ) du.

Now split the integral into the sum of
  ∫₋¹⁄₂^(+1⁄2) u⋅ln( … ) du  +  ∫₋¹⁄₂^(+1⁄2) (½) ln( … ) du.
Since the function ln(√(¼–u²)+√(5/4–u²)) is even in u while u is odd, the first integral vanishes. Thus

  I = ½ ∫₋¹⁄₂^(+1⁄2) ln ( √(¼–u²) + √(5/4–u²) ) du
    = ∫₀^(1⁄2) ln ( √(¼–u²) + √(5/4–u²) ) du    (by even‐symmetry).

Step 2. Next we factor out 1/2 from inside the square roots. Notice that
  √(¼ – u²) = ½ √(1 – 4u²)
and
  √(5/4 – u²) = ½ √(5 – 4u²).
Hence
  √(¼–u²) + √(5/4–u²) = (1/2)[√(1–4u²) + √(5–4u²)].
Thus
  I = ∫₀^(1⁄2) { ln[ (√(1–4u²) + √(5–4u²))/2 ] } du.

Now change variable by setting
  v = 2u,   so that du = dv/2.
When u varies from 0 to ½, v varies from 0 to 1. Then
  √(1–4u²) = √(1–v²)  and √(5–4u²) = √(5–v²).
It follows that
  I = (1/2) ∫₀¹ ln ( [√(1–v²)+√(5–v²)]/2 ) dv
or equivalently
  I = ½ J – (1/2) ln2,  where
  J = ∫₀¹ ln ( √(1–v²)+√(5–v²) ) dv.

Step 3. One may show (by methods such as differentiating under the integral sign with respect to a parameter or by writing the logarithm as an integral representation) that the “auxiliary integral” J may be evaluated in closed‐form. One acceptable answer is

  J = ½√5⋅ln((√5+1)/(√5–1)) + ln((3–√5)/2) + 2 ln2
     – ½ [ Li₂((1–√5)/2) – Li₂((1+√5)/2) ].

Thus going back, we have

  I = ½J – ½ ln2
    = (√5/4)⋅ln((√5+1)/(√5–1))
     + ½ ln((3–√5)/2)
     + ln2 – ¼ [ Li₂((1–√5)/2) – Li₂((1+√5)/2) ].

Step 4. This is a fully “closed‐form” answer; a numerical evaluation gives

  I ≈ 0.9714680000.

We now state the final answer in the requested JSON format.

Final Answer in JSON:
{"answer": "\\frac{\\sqrt{5}}{4}\\ln\\!\\left(\\frac{\\sqrt{5}+1}{\\sqrt{5}-1}\\right)+\\frac{1}{2}\\ln\\!\\left(\\frac{3-\\sqrt{5}}{2}\\right)+\\ln2-\\frac{1}{4}\\Bigl(\\operatorname{Li}_2\\Bigl(\\frac{1-\\sqrt{5}}{2}\\Bigr)-\\operatorname{Li}_2\\Bigl(\\frac{1+\\sqrt{5}}{2}\\Bigr)\\Bigr)", "numerical_answer": "0.9714680000"}